<?xml version="1.0" encoding="UTF-8"?>
  
<!DOCTYPE rdf:RDF [
    <!ENTITY fibo-be-ptr-ptr "http://spec.edmcouncil.org/fibo/red/be/partnerships/partnerships/">
    <!ENTITY fibo-fnd-acc-aeq "http://spec.edmcouncil.org/fibo/red/fnd/accounting/accounting-equity/">
    <!ENTITY fibo-be-le-fbo "http://spec.edmcouncil.org/fibo/red/be/legal-entities/formal-business-organizations/">
    <!ENTITY fibo-be-le-cb "http://spec.edmcouncil.org/fibo/red/be/legal-entities/corporate-bodies/">
    <!ENTITY fibo-be-oac-opty "http://spec.edmcouncil.org/fibo/red/be/ownership-and-control/ownership-parties/">
    <!ENTITY fibo-fnd-oac-own "http://spec.edmcouncil.org/fibo/red/fnd/ownership-and-control/ownership/">
    <!ENTITY fibo-fnd-law-lcap "http://spec.edmcouncil.org/fibo/red/fnd/law/legal-capacities/">
    <!ENTITY fibo-be-le-lp "http://spec.edmcouncil.org/fibo/red/be/legal-entities/legal-persons/">
    <!ENTITY fibo-fnd-pty-pty "http://spec.edmcouncil.org/fibo/red/fnd/parties/parties/">
    <!ENTITY fibo-fnd-agr-ctr "http://spec.edmcouncil.org/fibo/red/fnd/agreements/contracts/">
    <!ENTITY fibo-be-oac-cpty "http://spec.edmcouncil.org/fibo/red/be/ownership-and-control/control-parties/">
]>

<rdf:RDF xmlns:xsd="http://www.w3.org/2001/XMLSchema#"
         xmlns:sm="http://www.omg.org/techprocess/ab/SpecificationMetadata/"
         xmlns:xs="http://www.w3.org/2001/XMLSchema"
         xmlns:fibo-fnd-utl-av="http://www.omg.org/spec/EDMC-FIBO/FND/Utilities/AnnotationVocabulary/"
         xmlns:rdf="http://www.w3.org/1999/02/22-rdf-syntax-ns#"
         xmlns:rdfs="http://www.w3.org/2000/01/rdf-schema#"
         xmlns:owl="http://www.w3.org/2002/07/owl#"
         xmlns:skos="http://www.w3.org/2004/02/skos/core#"
         xmlns:dc="http://purl.org/dc/terms/"
         xml:base="http://spec.edmcouncil.org/fibo/red/be/partnerships/partnerships/">

   <owl:Ontology rdf:about="http://spec.edmcouncil.org/fibo/red/be/partnerships/partnerships/">
      <owl:imports rdf:resource="http://spec.edmcouncil.org/fibo/red/fnd/accounting/accounting-equity/"/>
      <owl:imports rdf:resource="http://spec.edmcouncil.org/fibo/red/be/legal-entities/formal-business-organizations/"/>
      <owl:imports rdf:resource="http://spec.edmcouncil.org/fibo/red/be/legal-entities/corporate-bodies/"/>
      <owl:imports rdf:resource="http://spec.edmcouncil.org/fibo/red/be/ownership-and-control/ownership-parties/"/>
      <owl:imports rdf:resource="http://spec.edmcouncil.org/fibo/red/fnd/ownership-and-control/ownership/"/>
      <owl:imports rdf:resource="http://spec.edmcouncil.org/fibo/red/fnd/law/legal-capacities/"/>
      <owl:imports rdf:resource="http://spec.edmcouncil.org/fibo/red/be/legal-entities/legal-persons/"/>
      <owl:imports rdf:resource="http://spec.edmcouncil.org/fibo/red/fnd/parties/parties/"/>
      <owl:imports rdf:resource="http://spec.edmcouncil.org/fibo/red/fnd/agreements/contracts/"/>
      <owl:imports rdf:resource="http://spec.edmcouncil.org/fibo/red/be/ownership-and-control/control-parties/"/>
   </owl:Ontology>


  <!--
    ///////////////////////////////////////////////////////////////////////////////////////
    //
    // Datatypes
    //
    ///////////////////////////////////////////////////////////////////////////////////////
    -->



  <!--
    ///////////////////////////////////////////////////////////////////////////////////////
    //
    // Object Properties
    //
    ///////////////////////////////////////////////////////////////////////////////////////
    -->


<owl:ObjectProperty rdf:about="&fibo-be-ptr-ptr;RepresentsAnInterestInPartnership">
      <rdfs:label>represents an interest in partnership</rdfs:label>
      <rdfs:subPropertyOf rdf:resource="&fibo-fnd-acc-aeq;equityRepresentsAnInterestIn"/>
      <rdfs:domain rdf:resource="&fibo-be-ptr-ptr;PartnershipEquity"/>
      <rdfs:range rdf:resource="&fibo-be-ptr-ptr;Partnership"/>
      <owl:inverseOf rdf:resource="&fibo-be-ptrx-ptrx;hasPartnershipEquity"/>
   </owl:ObjectProperty>

   <owl:ObjectProperty rdf:about="&fibo-be-ptr-ptr;corporateLimitedPartnerIdentity">
      <rdfs:label>corporate limited partner identity</rdfs:label>
      <skos:definition>That which is the Limited Partner. In this case, this can only be a Body Corporate.</skos:definition>
      <rdfs:subPropertyOf rdf:resource="&fibo-be-ptr-ptr;partnerIdentity"/>
      <rdfs:domain rdf:resource="&fibo-be-ptr-ptr;CorporateLimitedPartner"/>
      <rdfs:range rdf:resource="&fibo-be-le-cb;BodyCorporate"/>
   </owl:ObjectProperty>

   <owl:ObjectProperty rdf:about="&fibo-be-ptr-ptr;generalPartnerIdentity">
      <rdfs:label>general partner identity</rdfs:label>
      <skos:definition>That which is the General Partner.This can only be a Natural Person.</skos:definition>
      <rdfs:subPropertyOf rdf:resource="&fibo-be-ptr-ptr;partnerIdentity"/>
      <rdfs:domain rdf:resource="&fibo-be-ptr-ptr;GeneralPartner"/>
      <rdfs:range rdf:resource="&fibo-be-le-lp;NaturalPerson"/>
   </owl:ObjectProperty>

   <owl:ObjectProperty rdf:about="&fibo-be-ptr-ptr;hasMember">
      <rdfs:label>has member</rdfs:label>
      <skos:definition>A member or partner in the Partnership.</skos:definition>
      <rdfs:subPropertyOf rdf:resource="&fibo-be-ptr-ptr;hasPartner"/>
      <rdfs:domain rdf:resource="&fibo-be-ptr-ptr;LegallyIncorporatedPartnership"/>
      <rdfs:range rdf:resource="&fibo-be-ptr-ptr;LegallyIncorporatedPartnershipMember"/>
   </owl:ObjectProperty>

   <owl:ObjectProperty rdf:about="&fibo-be-ptr-ptr;naturalPersonLimitedPartnerIdentity">
      <rdfs:label>natural person limited partner identity</rdfs:label>
      <skos:definition>That which is the Limited Partner. In this case, this can only be a Natural Person.</skos:definition>
      <rdfs:subPropertyOf rdf:resource="&fibo-be-ptr-ptr;partnerIdentity"/>
      <rdfs:domain rdf:resource="&fibo-be-ptr-ptr;NaturalPersonLimitedPartner"/>
      <rdfs:range rdf:resource="&fibo-be-le-lp;NaturalPerson"/>
   </owl:ObjectProperty>

   <owl:ObjectProperty rdf:about="&fibo-be-ptr-ptr;partnerIdentity">
      <rdfs:label>partner identity</rdfs:label>
      <skos:definition>That which is the Partner.This is some Legal Person.</skos:definition>
      <rdfs:subPropertyOf rdf:resource="&fibo-fnd-pty-pty;hasIdentity"/>
      <rdfs:domain rdf:resource="&fibo-be-ptr-ptr;Partner"/>
      <rdfs:range rdf:resource="&fibo-be-le-lp;LegalPerson"/>
   </owl:ObjectProperty>

   <owl:ObjectProperty rdf:about="&fibo-be-ptr-ptr;partnershipAgreementHasParty">
      <rdfs:label>partnership agreement has party</rdfs:label>
      <skos:definition>The partnership agreement has the partners in the partnership as parties to that agreement.</skos:definition>
      <rdfs:subPropertyOf rdf:resource="&fibo-fnd-pty-pty;hasPartyInRole"/>
      <rdfs:domain rdf:resource="&fibo-be-ptr-ptr;PartnershipAgreement"/>
      <rdfs:range rdf:resource="&fibo-be-ptr-ptr;Partner"/>
   </owl:ObjectProperty>

   <owl:ObjectProperty rdf:about="&fibo-be-ptr-ptr;hasPartner">
      <rdfs:label>has partner</rdfs:label>
      <skos:definition>Any partner in the Partnership. Further notes: Note that nearly all partnerships have General Partners, and these are always present in non incorporated partnerships (but absent in limited liabilities companies which are otherwise styled as partnerships).</skos:definition>
      <rdfs:subPropertyOf rdf:resource="&fibo-fnd-pty-pty;hasPartyInRole"/>
      <rdfs:domain rdf:resource="&fibo-be-ptr-ptr;Partnership"/>
      <rdfs:range rdf:resource="&fibo-be-ptr-ptr;Partner"/>
   </owl:ObjectProperty>

   <owl:ObjectProperty rdf:about="&fibo-be-ptr-ptr;governedByPartnershipAgreement">
      <rdfs:label>governed by partnership agreement</rdfs:label>
      <skos:definition>The agreement between partners of the Partnership which governs the partnership as an entity.</skos:definition>
      <rdfs:subPropertyOf rdf:resource="&fibo-be-le-fbo;formallyConstitutedOrganizationIsGovernedBy"/>
      <rdfs:domain rdf:resource="&fibo-be-ptr-ptr;Partnership"/>
      <rdfs:range rdf:resource="&fibo-be-ptr-ptr;PartnershipAgreement"/>
   </owl:ObjectProperty>

   <owl:ObjectProperty rdf:about="&fibo-be-ptr-ptr;hasCapacityLiabilityCapacity">
      <rdfs:label>has capacity liability capacity</rdfs:label>
      <skos:definition>General Partner has some capacity for liability in respect to the debts or other liabilities incurred by the Partnership.</skos:definition>
      <rdfs:domain rdf:resource="&fibo-be-ptr-ptr;GeneralPartner"/>
      <rdfs:range rdf:resource="&fibo-fnd-law-lcap;LiabilityCapacity"/>
   </owl:ObjectProperty>

   <owl:ObjectProperty rdf:about="&fibo-be-ptr-ptr;hasCorporateLimitedPartner">
      <rdfs:label>has corporate limited partner</rdfs:label>
      <skos:definition>Has some Limited Partner which is a Body Corporate.</skos:definition>
      <rdfs:subPropertyOf rdf:resource="&fibo-be-ptr-ptr;hasLimitedPartner"/>
      <rdfs:domain rdf:resource="&fibo-be-ptr-ptr;PartnershipWithCorporateLimitedPartners"/>
      <rdfs:range rdf:resource="&fibo-be-ptr-ptr;CorporateLimitedPartner"/>
   </owl:ObjectProperty>

   <owl:ObjectProperty rdf:about="&fibo-be-ptr-ptr;hasGeneralPartner">
      <rdfs:label>has general partner</rdfs:label>
      <skos:definition>A General Partner in the partnership. This is some human person who is (jointly and severally with other such General Partners) liable for the debts of the partnership.</skos:definition>
      <rdfs:subPropertyOf rdf:resource="&fibo-be-ptr-ptr;hasPartner"/>
      <rdfs:domain rdf:resource="&fibo-be-ptr-ptr;PartnershipWithGeneralPartners"/>
      <rdfs:range rdf:resource="&fibo-be-ptr-ptr;GeneralPartner"/>
   </owl:ObjectProperty>

   <owl:ObjectProperty rdf:about="&fibo-be-ptr-ptr;hasLimitedPartner">
      <rdfs:label>has limited partner</rdfs:label>
      <skos:definition>Has one or more partners whose liabilities are limited.</skos:definition>
      <rdfs:subPropertyOf rdf:resource="&fibo-be-ptr-ptr;hasPartner"/>
      <rdfs:domain rdf:resource="&fibo-be-ptr-ptr;PartnershipWithLimitedPartners"/>
      <rdfs:range rdf:resource="&fibo-be-ptr-ptr;LimitedPartner"/>
   </owl:ObjectProperty>

   <owl:ObjectProperty rdf:about="&fibo-be-ptr-ptr;hasNaturalPersonLimitedPartner">
      <rdfs:label>has natural person limited partner</rdfs:label>
      <skos:definition>Has some Limited Partner which is a Natural Person.</skos:definition>
      <rdfs:subPropertyOf rdf:resource="&fibo-be-ptr-ptr;hasLimitedPartner"/>
      <rdfs:domain rdf:resource="&fibo-be-ptr-ptr;PartnershipWithNaturalPersonLimitedPartners"/>
      <rdfs:range rdf:resource="&fibo-be-ptr-ptr;NaturalPersonLimitedPartner"/>
   </owl:ObjectProperty>

   <owl:ObjectProperty rdf:about="&fibo-be-ptr-ptr;holdsGeneralPartnerEquity">
      <rdfs:label>holds general partner equity</rdfs:label>
      <skos:definition>General Partner equity held by the General Partner in the Partnership.</skos:definition>
      <rdfs:subPropertyOf rdf:resource="&fibo-be-ptr-ptr;holdsPartnershipEquity"/>
      <rdfs:domain rdf:resource="&fibo-be-ptr-ptr;GeneralPartner"/>
      <rdfs:range rdf:resource="&fibo-be-ptr-ptr;GeneralPartnerEquity"/>
   </owl:ObjectProperty>

   <owl:ObjectProperty rdf:about="&fibo-be-ptr-ptr;holdsLimitedPartnerEquity">
      <rdfs:label>holds limited partner equity</rdfs:label>
      <skos:definition>Limited Partner equity held by the Limited Partner in the Partnership.</skos:definition>
      <rdfs:subPropertyOf rdf:resource="&fibo-be-ptr-ptr;holdsPartnershipEquity"/>
      <rdfs:domain rdf:resource="&fibo-be-ptr-ptr;LimitedPartner"/>
      <rdfs:range rdf:resource="&fibo-be-ptr-ptr;LimitedPartnerEquity"/>
   </owl:ObjectProperty>

   <owl:ObjectProperty rdf:about="&fibo-be-ptr-ptr;holdsPartnershipEquity">
      <rdfs:label>holds partnership equity</rdfs:label>
      <skos:definition>The equity held by the Partner in the Partnership.</skos:definition>
      <rdfs:subPropertyOf rdf:resource="&fibo-be-oac-opty;holdsSomeStockholderEquity"/>
      <rdfs:subPropertyOf rdf:resource="&fibo-fnd-oac-own;owns"/>
      <rdfs:domain rdf:resource="&fibo-be-ptr-ptr;Partner"/>
      <rdfs:range rdf:resource="&fibo-be-ptr-ptr;PartnershipEquity"/>
   </owl:ObjectProperty>

   <owl:ObjectProperty rdf:about="&fibo-be-ptr-ptr;setsOutEquityTermsIn">
      <rdfs:label>sets out equity terms in</rdfs:label>
      <skos:definition>Has terms setting out the apportionment of equity in some Formal Business Organization.</skos:definition>
      <rdfs:subPropertyOf rdf:resource="&fibo-fnd-agr-ctr;contractHasTerms"/>
      <rdfs:domain rdf:resource="&fibo-be-le-fbo;OrganizationCoveringAgreement"/>
      <rdfs:range rdf:resource="&fibo-be-ptr-ptr;EquityApportionmentTermsSet"/>
   </owl:ObjectProperty>

   <owl:ObjectProperty rdf:about="&fibo-be-ptr-ptr;setsOutLiabilityTermsIn">
      <rdfs:label>sets out liability terms in</rdfs:label>
      <skos:definition>Has terms setting out the apportionment of liabilities for debts or other liabilities accrued by some Formal Business Organization.</skos:definition>
      <rdfs:subPropertyOf rdf:resource="&fibo-fnd-agr-ctr;contractHasTerms"/>
      <rdfs:domain rdf:resource="&fibo-be-le-fbo;OrganizationCoveringAgreement"/>
      <rdfs:range rdf:resource="&fibo-be-ptr-ptr;LiabilityApportionmentTermsSet"/>
   </owl:ObjectProperty>


  <!--
    ///////////////////////////////////////////////////////////////////////////////////////
    //
    // Data Properties
    //
    ///////////////////////////////////////////////////////////////////////////////////////
    -->


<owl:DatatypeProperty rdf:about="&fibo-be-ptr-ptr;dateOfIncorporation">
      <rdfs:label>date of incorporation</rdfs:label>
      <skos:definition>Date when the partnership was legally registered or incorporated as a distinct legal person.</skos:definition>
      <rdfs:range rdf:resource="http://www.w3.org/2001/XMLSchema#date"/>
   </owl:DatatypeProperty>

   <owl:DatatypeProperty rdf:about="&fibo-be-ptr-ptr;dateTradingFrom">
      <rdfs:label>date trading from</rdfs:label>
      <skos:definition>Date on which the Partnership started trading.</skos:definition>
      <rdfs:range rdf:resource="http://www.w3.org/2001/XMLSchema#date"/>
   </owl:DatatypeProperty>


  <!--
    ///////////////////////////////////////////////////////////////////////////////////////
    //
    // Annotation Properties
    //
    ///////////////////////////////////////////////////////////////////////////////////////
    -->



  <!--
    ///////////////////////////////////////////////////////////////////////////////////////
    //
    // Classes
    //
    ///////////////////////////////////////////////////////////////////////////////////////
    -->


<owl:Class rdf:about="&fibo-be-ptr-ptr;CorporateLimitedPartner">
      <rdfs:label>corporate limited partner</rdfs:label>
      <skos:definition>A limited partner in a partnership, who is and may only be a Corporate Legal Person i.e. not a human being.</skos:definition>
      <rdfs:subClassOf rdf:resource="&fibo-be-ptr-ptr;LimitedPartner"/>
   </owl:Class>

   <owl:Class rdf:about="&fibo-be-ptr-ptr;EquityApportionmentTermsSet">
      <rdfs:label>equity apportionment terms set</rdfs:label>
      <skos:definition>Terms setting out the apportionment of equity in some Formal Organization.</skos:definition>
   </owl:Class>

   <owl:Class rdf:about="&fibo-be-ptr-ptr;GeneralPartner">
      <rdfs:label>general partner</rdfs:label>
      <skos:definition>A partner in a partnership, who holds some part of the general partner equity and typically is jointly and severally liable with the other partners for the liabilities incurred by that partnership.</skos:definition>
      <rdfs:subClassOf rdf:resource="&fibo-be-oac-cpty;DeJureControllingInterestParty"/>
      <rdfs:subClassOf rdf:resource="&fibo-be-ptr-ptr;Partner"/>
   </owl:Class>

   <owl:Class rdf:about="&fibo-be-ptr-ptr;GeneralPartnerEquity">
      <rdfs:label>general partner equity</rdfs:label>
      <skos:definition>Equity in a partnership held by General Partners. This is typically accompanied by full liability capability on the part of the holders of the equity.</skos:definition>
      <rdfs:subClassOf rdf:resource="&fibo-be-oac-opty;ControllingEquity"/>
      <rdfs:subClassOf rdf:resource="&fibo-be-ptr-ptr;PartnershipEquity"/>
   </owl:Class>

   <owl:Class rdf:about="&fibo-be-ptr-ptr;LegallyIncorporatedPartnership">
      <rdfs:label>legally incorporated partnership</rdfs:label>
      <skos:definition>Any partnership which is defined as a legal person within a given Jurisdiction, for example a Limited Liability Partnership (if that is a legal person).</skos:definition>
      <rdfs:subClassOf rdf:resource="&fibo-be-le-cb;BodyCorporate"/>
      <rdfs:subClassOf rdf:resource="&fibo-be-ptr-ptr;Partnership"/>
   </owl:Class>

   <owl:Class rdf:about="&fibo-be-ptr-ptr;LegallyIncorporatedPartnershipMember">
      <rdfs:label>legally incorporated partnership member</rdfs:label>
      <skos:definition>A party which is a member or partner in a Legally Incorporated Partnership such as an LLC or LLP.</skos:definition>
   </owl:Class>

   <owl:Class rdf:about="&fibo-be-ptr-ptr;LiabilityApportionmentTermsSet">
      <rdfs:label>liability apportionment terms set</rdfs:label>
      <skos:definition>Terms setting out the apportionment of liabilities for debts or other liabilities accrued by some Formal Organization.</skos:definition>
   </owl:Class>

   <owl:Class rdf:about="&fibo-be-ptr-ptr;LimitedPartner">
      <rdfs:label>limited partner</rdfs:label>
      <skos:definition>A partner in a partnership whose liabilities are limited to the extent of their equity holding or guarantees.</skos:definition>
   </owl:Class>

   <owl:Class rdf:about="&fibo-be-ptr-ptr;LimitedPartnerEquity">
      <rdfs:label>limited partner equity</rdfs:label>
      <rdfs:subClassOf rdf:resource="&fibo-fnd-acc-aeq;IssuedEquity"/>
   </owl:Class>

   <owl:Class rdf:about="&fibo-be-ptr-ptr;NaturalPersonLimitedPartner">
      <rdfs:label>natural person limited partner</rdfs:label>
      <skos:definition>A limited partner in a partnership, who is and may only be a Natural Person i.e. a human being.</skos:definition>
   </owl:Class>

   <owl:Class rdf:about="&fibo-be-ptr-ptr;NonIncorporatedPartnership">
      <rdfs:label>non incorporated partnership</rdfs:label>
      <rdfs:subClassOf rdf:resource="&fibo-be-ptr-ptr;PartnershipWithGeneralPartners"/>
   </owl:Class>

   <owl:Class rdf:about="&fibo-be-ptr-ptr;Partner">
      <rdfs:label>partner</rdfs:label>
      <skos:definition>Any partner in a Partnership. Scope Note: This term is not referred to directly in specific kinds of partnership. Nearly all partnerships have General Partners, while forms of (mostly legally incorporated) partnerships have in addition Limited Partners. This term is the common ancestor of both.</skos:definition>
      <rdfs:subClassOf rdf:resource="&fibo-be-le-fbo;FormalBusinessOrganizationMember"/>
      <rdfs:subClassOf rdf:resource="&fibo-be-oac-opty;ConstitutionalOwner"/>
   </owl:Class>

   <owl:Class rdf:about="&fibo-be-ptr-ptr;Partnership">
      <rdfs:label>partnership</rdfs:label>
      <skos:definition>Venture in which two or more legal entities carry out some business activities under a common identity.</skos:definition>
      <rdfs:subClassOf rdf:resource="&fibo-be-le-fbo;FormallyConstitutedOrganization"/>
   </owl:Class>

   <owl:Class rdf:about="&fibo-be-ptr-ptr;PartnershipAgreement">
      <rdfs:label>partnership agreement</rdfs:label>
      <skos:definition>The agreement between partners of the Partnership.</skos:definition>
      <rdfs:subClassOf rdf:resource="&fibo-be-le-fbo;OrganizationCoveringAgreement"/>
   </owl:Class>

   <owl:Class rdf:about="&fibo-be-ptr-ptr;PartnershipEquity">
      <rdfs:label>partnership equity</rdfs:label>
      <skos:definition>Equity in some Partnership.</skos:definition>
      <rdfs:subClassOf rdf:resource="&fibo-fnd-acc-aeq;StockholdersEquity"/>
   </owl:Class>

   <owl:Class rdf:about="&fibo-be-ptr-ptr;PartnershipIncorporatedByEquity">
      <rdfs:label>partnership incorporated by equity</rdfs:label>
      <rdfs:subClassOf rdf:resource="&fibo-be-le-cb;BodyIncorporatedWithEquity"/>
      <rdfs:subClassOf rdf:resource="&fibo-be-ptr-ptr;PartnershipWithLimitedPartners"/>
   </owl:Class>

   <owl:Class rdf:about="&fibo-be-ptr-ptr;PartnershipIncorporatedThroughAgreement">
      <rdfs:label>partnership incorporated through agreement</rdfs:label>
      <skos:definition>A partnership which has legal personhood, but for which there is not some issuance of limited partner equity.</skos:definition>
      <rdfs:subClassOf rdf:resource="&fibo-be-le-cb;BodyIncorporatedThroughAgreement"/>
   </owl:Class>

   <owl:Class rdf:about="&fibo-be-ptr-ptr;PartnershipWithCorporateLimitedPartners">
      <rdfs:label>partnership with corporate limited partners</rdfs:label>
   </owl:Class>

   <owl:Class rdf:about="&fibo-be-ptr-ptr;PartnershipWithGeneralAndLimitedPartners">
      <rdfs:label>partnership with general and limited partners</rdfs:label>
      <skos:definition>A partnership having both limited partners nd general partners.</skos:definition>
   </owl:Class>

   <owl:Class rdf:about="&fibo-be-ptr-ptr;PartnershipWithGeneralPartners">
      <rdfs:label>partnership with general partners</rdfs:label>
      <skos:definition>A partnership which has two or more General Partners.</skos:definition>
   </owl:Class>

   <owl:Class rdf:about="&fibo-be-ptr-ptr;PartnershipWithGeneralPartnersWithLimitedLiability">
      <rdfs:label>partnership with general partners with limited liability</rdfs:label>
      <skos:definition>A partnership that has General Partners, but where those General Partners have limited liability.</skos:definition>
   </owl:Class>

   <owl:Class rdf:about="&fibo-be-ptr-ptr;PartnershipWithLimitedPartners">
      <rdfs:label>partnership with limited partners</rdfs:label>
      <skos:definition>A partnership having Limited Partners, that is partners whose liabilities are limited to the extent of their equity or guarantees.</skos:definition>
   </owl:Class>

   <owl:Class rdf:about="&fibo-be-ptr-ptr;PartnershipWithNaturalPersonLimitedPartners">
      <rdfs:label>partnership with natural person limited partners</rdfs:label>
      <skos:definition>A partnership with limited partners (partners whose liability is limited) and where those partners are necessarily natural persons (i.e. cannot be corporates). Scope Note: Example in US: "Limited Liability Partnership"</skos:definition>
   </owl:Class>

   <owl:Class rdf:about="&fibo-be-ptr-ptr;PartnershipWithOnlyLimitedPartners">
      <rdfs:label>partnership with only limited partners</rdfs:label>
   </owl:Class>


  <!--
    ///////////////////////////////////////////////////////////////////////////////////////
    //
    // Individuals
    //
    ///////////////////////////////////////////////////////////////////////////////////////
    -->


</rdf:RDF>