<?xml version="1.0" encoding="UTF-8"?>
<rdf:RDF xmlns:xsd="http://www.w3.org/2001/XMLSchema#"
         xmlns:sm="http://www.omg.org/techprocess/ab/SpecificationMetadata/"
         xmlns:fibo-fnd-utl-av="http://www.omg.org/spec/EDMC-FIBO/FND/Utilities/AnnotationVocabulary/"
         xmlns:rdf="http://www.w3.org/1999/02/22-rdf-syntax-ns#"
         xmlns:rdfs="http://www.w3.org/2000/01/rdf-schema#"
         xmlns:owl="http://www.w3.org/2002/07/owl#"
         xmlns:skos="http://www.w3.org/2004/02/skos/core#"
         xmlns:dc="http://purl.org/dc/terms/"
         xml:base="http://www.omg.org/spec/EDMC-SR/FND/Agreements/Agreements/">

   <owl:Ontology rdf:about="http://www.omg.org/spec/EDMC-SR/FND/Agreements/Agreements/">
      <owl:imports rdf:resource="http://www.edmcouncil.org/spec/EDMC-SR/FND/SocialConstructs/SocialConstructs/"/>
      <owl:imports rdf:resource="http://www.edmcouncil.org/spec/EDMC-SR/UO/Lattice/"/>
      <owl:imports rdf:resource="http://www.omg.org/spec/EDMC-SR/FND/Parties/Parties/"/>
   </owl:Ontology>

   <!--Datatypes-->

<!--Object Properties-->

<owl:ObjectProperty rdf:about="http://www.omg.org/spec/EDMC-SR/FND/Agreements/Agreements/agreementHasPartyInRole">
      <skos:definition>A party to the Agreement.</skos:definition>
      <rdfs:subPropertyOf rdf:resource="http://www.omg.org/spec/EDMC-SR/FND/Parties/Parties/hasPartyInRole"/>
      <rdfs:domain rdf:resource="http://www.omg.org/spec/EDMC-SR/FND/Agreements/Agreements/Agreement"/>
      <rdfs:range rdf:resource="http://www.omg.org/spec/EDMC-SR/FND/Parties/Parties/PartyInRole"/>
   </owl:ObjectProperty>

   <owl:ObjectProperty rdf:about="http://www.omg.org/spec/EDMC-SR/FND/Agreements/Agreements/bilateralAgreementHasPartyInRole">
      <skos:definition>A party to the Bilateral Agreement. There are exactly two of parties to the Agreement.</skos:definition>
      <rdfs:subPropertyOf rdf:resource="http://www.omg.org/spec/EDMC-SR/FND/Parties/Parties/hasPartyInRole"/>
      <rdfs:domain rdf:resource="http://www.omg.org/spec/EDMC-SR/FND/Agreements/Agreements/BilateralAgreement"/>
      <rdfs:range rdf:resource="http://www.omg.org/spec/EDMC-SR/FND/Parties/Parties/PartyInRole"/>
   </owl:ObjectProperty>

   <owl:ObjectProperty rdf:about="http://www.omg.org/spec/EDMC-SR/FND/Agreements/Agreements/multilateralAgreementHasPartyInRole">
      <skos:definition>A party to the Multilateral Agreement. There are at least three parties to the Agreement,</skos:definition>
      <rdfs:subPropertyOf rdf:resource="http://www.omg.org/spec/EDMC-SR/FND/Parties/Parties/hasPartyInRole"/>
      <rdfs:domain rdf:resource="http://www.omg.org/spec/EDMC-SR/FND/Agreements/Agreements/MultilateralAgreement"/>
      <rdfs:range rdf:resource="http://www.omg.org/spec/EDMC-SR/FND/Parties/Parties/PartyInRole"/>
   </owl:ObjectProperty>

   <owl:ObjectProperty rdf:about="http://www.omg.org/spec/EDMC-SR/FND/Agreements/Agreements/confersCommitment">
      <skos:definition>Some Commitment which arises from the Agreement and exists as a result of that Agreement.</skos:definition>
      <rdfs:subPropertyOf rdf:resource="http://www.omg.org/spec/EDMC-SR/FND/Relations/Relations/confers"/>
      <rdfs:domain rdf:resource="http://www.omg.org/spec/EDMC-SR/FND/Agreements/Agreements/Agreement"/>
      <rdfs:range rdf:resource="http://www.omg.org/spec/EDMC-SR/FND/Agreements/Agreements/MutualCommitment"/>
   </owl:ObjectProperty>

   <!--Data Properties-->

<!--Annotation Properties-->

<!--Classes-->

<owl:Class rdf:about="http://www.omg.org/spec/EDMC-SR/FND/Agreements/Agreements/Agreement">
      <rdfs:label>Agreement</rdfs:label>
      <skos:definition>Some mutual undertaking or set of undertakings between two or among several parties.</skos:definition>
      <skos:editorialNote>An Agreement may be formalized in the form of a Contract or other formal instrument, or it may not. In either case, the agreement is that which may be referred to as the agreement between or among the parties, and the contract is framed as defining (and usually as exclusively defining) the agreement between two parties.</skos:editorialNote>
      <rdfs:subClassOf rdf:resource="http://www.edmcouncil.org/spec/EDMC-SR/UO/Lattice/Abstract"/>
      <rdfs:subClassOf rdf:resource="http://www.edmcouncil.org/spec/EDMC-SR/FND/Relative/PartyRoleContext/RelationshipContext"/>
   </owl:Class>

   <owl:Class rdf:about="http://www.omg.org/spec/EDMC-SR/FND/Agreements/Agreements/BilateralAgreement">
      <rdfs:label>Bilateral Agreement</rdfs:label>
      <skos:definition>Some Agreement which is between two parties.</skos:definition>
      <rdfs:subClassOf rdf:resource="http://www.omg.org/spec/EDMC-SR/FND/Agreements/Agreements/Agreement"/>
   </owl:Class>

   <owl:Class rdf:about="http://www.omg.org/spec/EDMC-SR/FND/Agreements/Agreements/Commitment">
      <rdfs:label>Commitment</rdfs:label>
      <skos:definition>A legal construct which represent the undertaking on the part of some party to act or refrain from acting in some manner.</skos:definition>
      <skos:editorialNote>The undertaking by some party to act or refrain from acting results in an obligation on the part of that party, and usually results in the existence of some corresponding right on the party of some other party, in the event that the commitment is to such party. Thus Obligations and Rights are considered as reciprocal aspects of this Commitment concept.</skos:editorialNote>
      <rdfs:subClassOf rdf:resource="http://www.edmcouncil.org/spec/EDMC-SR/FND/SocialConstructs/SocialConstructs/SocialConstruct"/>
   </owl:Class>

   <owl:Class rdf:about="http://www.omg.org/spec/EDMC-SR/FND/Agreements/Agreements/MultilateralAgreement">
      <rdfs:label>Multilateral Agreement</rdfs:label>
      <skos:definition>An agreement between three or more parties</skos:definition>
   </owl:Class>

   <owl:Class rdf:about="http://www.omg.org/spec/EDMC-SR/FND/Agreements/Agreements/MutualCommitment">
      <rdfs:label>Mutual Commitment</rdfs:label>
      <skos:definition>A commitment undertaken as between two parties.</skos:definition>
      <rdfs:subClassOf rdf:resource="http://www.omg.org/spec/EDMC-SR/FND/Agreements/Agreements/Commitment"/>
   </owl:Class>

   <owl:Class rdf:about="http://www.omg.org/spec/EDMC-SR/FND/Agreements/Agreements/UniteralCommitment">
      <rdfs:label>Uniteral Commitment</rdfs:label>
      <skos:definition>A commitment made by one party without reference to the party to which the commitment is made.</skos:definition>
   </owl:Class>

   <!--Individuals-->

</rdf:RDF>