<?xml version="1.0" encoding="UTF-8"?>
<rdf:RDF xmlns:xsd="http://www.w3.org/2001/XMLSchema#"
         xmlns:sm="http://www.omg.org/techprocess/ab/SpecificationMetadata/"
         xmlns:fibo-fnd-utl-av="http://www.omg.org/spec/EDMC-FIBO/FND/Utilities/AnnotationVocabulary/"
         xmlns:rdf="http://www.w3.org/1999/02/22-rdf-syntax-ns#"
         xmlns:rdfs="http://www.w3.org/2000/01/rdf-schema#"
         xmlns:owl="http://www.w3.org/2002/07/owl#"
         xmlns:skos="http://www.w3.org/2004/02/skos/core#"
         xmlns:dc="http://purl.org/dc/terms/"
         xml:base="http://www.omg.org/spec/EDMC-SR/FND/Agreements/Contracts/">

   <owl:Ontology rdf:about="http://www.omg.org/spec/EDMC-SR/FND/Agreements/Contracts/">
      <owl:imports rdf:resource="http://www.omg.org/spec/EDMC-SR/FND/Law/LegalCore/"/>
      <owl:imports rdf:resource="http://www.omg.org/spec/EDMC-SR/FND/Agreements/Agreements/"/>
   </owl:Ontology>

   <!--Datatypes-->

<!--Object Properties-->

<owl:ObjectProperty rdf:about="http://www.omg.org/spec/EDMC-SR/FND/Agreements/Contracts/bilateralContractHasPartyInRole">
      <rdfs:subPropertyOf rdf:resource="http://www.omg.org/spec/EDMC-SR/FND/Parties/Parties/hasPartyInRole"/>
      <rdfs:domain rdf:resource="http://www.omg.org/spec/EDMC-SR/FND/Agreements/Contracts/BilateralContract"/>
      <rdfs:range rdf:resource="http://www.omg.org/spec/EDMC-SR/FND/Parties/Parties/PartyInRole"/>
   </owl:ObjectProperty>

   <owl:ObjectProperty rdf:about="http://www.omg.org/spec/EDMC-SR/FND/Agreements/Contracts/contractTermsSetHasPart">
      <skos:definition>A set of terms which forms part of the contract terms set. This may be a sub-clause, a clause or simply another definition of a set of terms at a smaller granularity than the set from which these are referred.</skos:definition>
      <rdfs:subPropertyOf rdf:resource="http://www.omg.org/spec/EDMC-SR/FND/Relations/Relations/hasPart"/>
      <rdfs:domain rdf:resource="http://www.omg.org/spec/EDMC-SR/FND/Agreements/Contracts/ContractTermsSet"/>
      <rdfs:range rdf:resource="http://www.omg.org/spec/EDMC-SR/FND/Agreements/Contracts/ContractTermsSet"/>
   </owl:ObjectProperty>

   <owl:ObjectProperty rdf:about="http://www.omg.org/spec/EDMC-SR/FND/Agreements/Contracts/contractHasTerms">
      <skos:definition>A set of terms that form part of the contract.</skos:definition>
      <skos:editorialNote>These are generally grouped for convenience in defining terms, such as debt repayment terms, and may or may not equate to a formal clause, section, paragraph or other textual construct of the contract.</skos:editorialNote>
      <rdfs:domain rdf:resource="http://www.omg.org/spec/EDMC-SR/FND/Agreements/Contracts/Contract"/>
      <rdfs:range rdf:resource="http://www.omg.org/spec/EDMC-SR/FND/Agreements/Contracts/ContractTermsSet"/>
   </owl:ObjectProperty>

   <owl:ObjectProperty rdf:about="http://www.omg.org/spec/EDMC-SR/FND/Agreements/Contracts/contractHasPartyInRole">
      <rdfs:subPropertyOf rdf:resource="http://www.omg.org/spec/EDMC-SR/FND/Parties/Parties/hasPartyInRole"/>
      <rdfs:domain rdf:resource="http://www.omg.org/spec/EDMC-SR/FND/Agreements/Contracts/Contract"/>
      <rdfs:range rdf:resource="http://www.omg.org/spec/EDMC-SR/FND/Parties/Parties/PartyInRole"/>
   </owl:ObjectProperty>

   <owl:ObjectProperty rdf:about="http://www.omg.org/spec/EDMC-SR/FND/Agreements/Contracts/definesTermsFor">
      <skos:definition>the contract sets out the terms for the something</skos:definition>
      <rdfs:domain rdf:resource="http://www.omg.org/spec/EDMC-SR/FND/Agreements/Contracts/Contract"/>
      <rdfs:range rdf:resource="http://www.w3.org/2002/07/owl#Thing"/>
   </owl:ObjectProperty>

   <owl:ObjectProperty rdf:about="http://www.omg.org/spec/EDMC-SR/FND/Agreements/Contracts/hasCounterparty">
      <skos:definition>The second party to a contract. In the event that the contract identifies either party as being the principal, this is the other party to that contract.</skos:definition>
      <rdfs:subPropertyOf rdf:resource="http://www.edmcouncil.org/spec/EDMC-SR/FND/AgreementsExt/ContractsExtensions/hasParty"/>
      <rdfs:subPropertyOf rdf:resource="http://www.omg.org/spec/EDMC-SR/FND/Parties/Parties/hasPartyInRole"/>
      <rdfs:domain rdf:resource="http://www.omg.org/spec/EDMC-SR/FND/Agreements/Contracts/Contract"/>
      <rdfs:range rdf:resource="http://www.omg.org/spec/EDMC-SR/FND/Agreements/Contracts/ContractCounterparty"/>
   </owl:ObjectProperty>

   <owl:ObjectProperty rdf:about="http://www.omg.org/spec/EDMC-SR/FND/Agreements/Contracts/hasGoverningJurisdiction">
      <skos:definition>The jurisdiction under which the contract is governed, as agreed by both parties. In a written contract this is generally identified in a clause identified for example as Governing Law. This is the jurisdiction under which any disputes arising from the contract are to be resolved.</skos:definition>
      <skos:editorialNote>As currently modeled this relationship combines two slightly different senses in which a Jurisdiction may be named in some Contract: the jurisdiction under whose laws the contract is deemed to be in force, and the jurisdiction under which the parties agree to submit in the event of any dispute resolution. Scope Note: One thing to tease out is whether "Dispute Resolution" and other forms of "Governing Law" are one and the same thing or not. Dispute Resolution is uncontroversial, the question is whether there are other implications to Governing Law or if it's the same thing. For instance I may undertake to behave as though I were responsible to a particular authority i.e. a particular set of statutes.</skos:editorialNote>
      <rdfs:subPropertyOf rdf:resource="http://www.omg.org/spec/EDMC-SR/FND/Relations/Relations/isGoverneBy"/>
      <rdfs:domain rdf:resource="http://www.omg.org/spec/EDMC-SR/FND/Agreements/Contracts/Contract"/>
      <rdfs:range rdf:resource="http://www.omg.org/spec/EDMC-SR/FND/Law/Jurisdictions/Jurisdiction"/>
   </owl:ObjectProperty>

   <owl:ObjectProperty rdf:about="http://www.omg.org/spec/EDMC-SR/FND/Agreements/Contracts/hasNonBindingTerms">
      <skos:definition>Terms which are included in the contract but are not considered binding. A breach of such terms in the future would not be considered to be a breach of the contract.</skos:definition>
      <rdfs:subPropertyOf rdf:resource="http://www.omg.org/spec/EDMC-SR/FND/Agreements/Contracts/contractHasTerms"/>
      <rdfs:domain rdf:resource="http://www.omg.org/spec/EDMC-SR/FND/Agreements/Contracts/Contract"/>
      <rdfs:range rdf:resource="http://www.omg.org/spec/EDMC-SR/FND/Agreements/Contracts/NonBindingTermsSet"/>
   </owl:ObjectProperty>

   <owl:ObjectProperty rdf:about="http://www.omg.org/spec/EDMC-SR/FND/Agreements/Contracts/hasPrincipal">
      <skos:definition>The main or principal party to the contract, if either party is identified as such.</skos:definition>
      <rdfs:subPropertyOf rdf:resource="http://www.edmcouncil.org/spec/EDMC-SR/FND/AgreementsExt/ContractsExtensions/hasParty"/>
      <rdfs:subPropertyOf rdf:resource="http://www.omg.org/spec/EDMC-SR/FND/Parties/Parties/hasPartyInRole"/>
      <rdfs:domain rdf:resource="http://www.omg.org/spec/EDMC-SR/FND/Agreements/Contracts/Contract"/>
      <rdfs:range rdf:resource="http://www.omg.org/spec/EDMC-SR/FND/Agreements/Contracts/ContractPrincipal"/>
   </owl:ObjectProperty>

   <owl:ObjectProperty rdf:about="http://www.omg.org/spec/EDMC-SR/FND/Agreements/Contracts/hasThirdParty">
      <skos:definition>A party which is not signatory to the party but has some role in the overall context defined by the contract.</skos:definition>
      <rdfs:subPropertyOf rdf:resource="http://www.omg.org/spec/EDMC-SR/FND/Parties/Parties/hasPartyInRole"/>
      <rdfs:subPropertyOf rdf:resource="http://www.edmcouncil.org/spec/EDMC-SR/FND/AgreementsExt/ContractsExtensions/hasParty"/>
      <rdfs:domain rdf:resource="http://www.omg.org/spec/EDMC-SR/FND/Agreements/Contracts/Contract"/>
      <rdfs:range rdf:resource="http://www.omg.org/spec/EDMC-SR/FND/Agreements/Contracts/ContractThirdParty"/>
   </owl:ObjectProperty>

   <owl:ObjectProperty rdf:about="http://www.omg.org/spec/EDMC-SR/FND/Agreements/Contracts/heldBy">
      <skos:definition>The anonymous counterparty that holds the contract and may transfer the rights and obligations therein to another such holder.</skos:definition>
      <rdfs:subPropertyOf rdf:resource="http://www.omg.org/spec/EDMC-SR/FND/Agreements/Contracts/hasCounterparty"/>
      <rdfs:domain rdf:resource="http://www.omg.org/spec/EDMC-SR/FND/Agreements/Contracts/TransferableContract"/>
      <rdfs:range rdf:resource="http://www.omg.org/spec/EDMC-SR/FND/Agreements/Contracts/TransferableContractHolder"/>
   </owl:ObjectProperty>

   <owl:ObjectProperty rdf:about="http://www.omg.org/spec/EDMC-SR/FND/Agreements/Contracts/writtenBy">
      <skos:definition>The party by whom the transferable contract has been written.</skos:definition>
      <rdfs:subPropertyOf rdf:resource="http://www.omg.org/spec/EDMC-SR/FND/Agreements/Contracts/hasPrincipal"/>
      <rdfs:domain rdf:resource="http://www.omg.org/spec/EDMC-SR/FND/Agreements/Contracts/TransferableContract"/>
      <rdfs:range rdf:resource="http://www.omg.org/spec/EDMC-SR/FND/Agreements/Contracts/ContractOriginator"/>
   </owl:ObjectProperty>

   <owl:ObjectProperty rdf:about="http://www.omg.org/spec/EDMC-SR/FND/Agreements/Contracts/supersedes">
      <skos:definition>The or any earlier contract which this written contract supersedes, whether that earlier contract is written or verbal or implied.</skos:definition>
      <rdfs:domain rdf:resource="http://www.omg.org/spec/EDMC-SR/FND/Agreements/Contracts/WrittenContract"/>
      <rdfs:range rdf:resource="http://www.omg.org/spec/EDMC-SR/FND/Agreements/Contracts/Contract"/>
   </owl:ObjectProperty>

   <!--Data Properties-->

<owl:DatatypeProperty rdf:about="http://www.omg.org/spec/EDMC-SR/FND/Agreements/Contracts/hasEffectiveDate">
      <rdfs:range rdf:resource="http://www.w3.org/2001/XMLSchema#date"/>
   </owl:DatatypeProperty>

   <owl:DatatypeProperty rdf:about="http://www.omg.org/spec/EDMC-SR/FND/Agreements/Contracts/isAssignable">
      <rdfs:range rdf:resource="http://www.omg.org/spec/EDMC-SR/FND/Utilities/BusinessFacingTypes/yesOrNo"/>
   </owl:DatatypeProperty>

   <!--Annotation Properties-->

<!--Classes-->

<owl:Class rdf:about="http://www.omg.org/spec/EDMC-SR/FND/Agreements/Contracts/ConditionsPrecedent">
      <rdfs:label>Conditions Precedent</rdfs:label>
      <skos:definition>Conditions precedent on some obligation. These are conditions which would alter the Obligation as it is otherwise stated.</skos:definition>
      <skos:editorialNote>Introduced for ISDA Master Agreement. It is likely that the Conditions Precedent defined for OTC Derivatives Master Agreements are actually applicable more widely. However, they are defined within the ISDA terms for now. Modeling note / review question: Modeled as a kind of Terms Set, combining terms and conditions. Should consider whether terms and conditions are distinct (Condition would then be a separate archetype).</skos:editorialNote>
      <rdfs:subClassOf rdf:resource="http://www.omg.org/spec/EDMC-SR/FND/Agreements/Contracts/ContractTermsSet"/>
   </owl:Class>

   <owl:Class rdf:about="http://www.omg.org/spec/EDMC-SR/FND/Agreements/Contracts/Contract">
      <rdfs:label>Contract</rdfs:label>
      <rdfs:subClassOf rdf:resource="http://www.edmcouncil.org/spec/EDMC-SR/UO/Lattice/ContinuantThing"/>
      <rdfs:subClassOf rdf:resource="http://www.edmcouncil.org/spec/EDMC-SR/UO/Lattice/Concrete"/>
      <rdfs:subClassOf rdf:resource="http://www.edmcouncil.org/spec/EDMC-SR/FND/Relative/PartyRoleContext/RelationshipContext"/>
   </owl:Class>

   <owl:Class rdf:about="http://www.omg.org/spec/EDMC-SR/FND/Agreements/Contracts/ContractCounterparty">
      <rdfs:label>Contract Counterparty</rdfs:label>
      <rdfs:subClassOf rdf:resource="http://www.edmcouncil.org/spec/EDMC-SR/FND/AgreementsExt/ContractsExtensions/ContractParty"/>
      <rdfs:subClassOf rdf:resource="http://www.omg.org/spec/EDMC-SR/FND/Parties/Parties/PartyInRole"/>
   </owl:Class>

   <owl:Class rdf:about="http://www.omg.org/spec/EDMC-SR/FND/Agreements/Contracts/ContractPrincipal">
      <rdfs:label>Contract Principal</rdfs:label>
      <skos:definition>The party identified as being the principal or first party to a contract, in the event that the contract distinguishes either party as being the principal.</skos:definition>
   </owl:Class>

   <owl:Class rdf:about="http://www.omg.org/spec/EDMC-SR/FND/Agreements/Contracts/ContractTermsSet">
      <rdfs:label>Contract Terms Set</rdfs:label>
      <rdfs:subClassOf rdf:resource="http://www.edmcouncil.org/spec/EDMC-SR/FND/Relative/SetMembership/Set"/>
      <rdfs:subClassOf rdf:resource="http://www.omg.org/spec/EDMC-SR/FND/Agreements/Contracts/ContractualElement"/>
   </owl:Class>

   <owl:Class rdf:about="http://www.omg.org/spec/EDMC-SR/FND/Agreements/Contracts/ContractThirdParty">
      <rdfs:label>Contract Third Party</rdfs:label>
      <skos:definition>A party which is identified in a contract but which is not itself party to that contract.</skos:definition>
   </owl:Class>

   <owl:Class rdf:about="http://www.omg.org/spec/EDMC-SR/FND/Agreements/Contracts/ContractualDefinition">
      <rdfs:label>Contractual Definition</rdfs:label>
      <skos:definition>The definition of something in some contract or other legal instrument.</skos:definition>
      <skos:editorialNote>These are agreed definitions which are then referred to in terms in contracts or other legal instruments.</skos:editorialNote>
   </owl:Class>

   <owl:Class rdf:about="http://www.omg.org/spec/EDMC-SR/FND/Agreements/Contracts/ContractualElement">
      <rdfs:label>Contractual Element</rdfs:label>
      <skos:definition>Anything which relates to contracts.</skos:definition>
   </owl:Class>

   <owl:Class rdf:about="http://www.omg.org/spec/EDMC-SR/FND/Agreements/Contracts/ContractualRelationship">
      <rdfs:label>Contractual Relationship</rdfs:label>
      <skos:definition>A relationship in which two or more parties have some contractual obligations or extend some rights under a contract, to one another.</skos:definition>
   </owl:Class>

   <owl:Class rdf:about="http://www.omg.org/spec/EDMC-SR/FND/Agreements/Contracts/NonBindingTermsSet">
      <rdfs:label>Non Binding Terms Set</rdfs:label>
      <skos:definition>Terms which do not have binding legal standing on the Issuer or Holder.</skos:definition>
   </owl:Class>

   <owl:Class rdf:about="http://www.omg.org/spec/EDMC-SR/FND/Agreements/Contracts/PromissoryNote">
      <rdfs:label>Promissory Note</rdfs:label>
      <skos:definition>A promise by the issuer of the note, of some good or benefit to the holder.</skos:definition>
      <skos:editorialNote>Unlike a contract, a Promissory Note does not need to be signed by both parties. It is essentiually a promise from one party to the holder, of some good or benefit. Promissory notes would generally by fully fungible. These are modeled as a kind of contract but are essentially a kind of unilateral contract between the issuer and the holder, and some authorities might not see this as a contract at all. Cash is a kind of promissory note, with the issuer being a central bank.</skos:editorialNote>
      <rdfs:subClassOf rdf:resource="http://www.omg.org/spec/EDMC-SR/FND/Agreements/Contracts/WrittenContract"/>
   </owl:Class>

   <owl:Class rdf:about="http://www.omg.org/spec/EDMC-SR/FND/Agreements/Contracts/TransferableContractHolder">
      <rdfs:label>Transferable Contract Holder</rdfs:label>
      <skos:definition>The party which holds a transferable contract and enjoys the benefits defined in that contract while they hold it.</skos:definition>
      <skos:editorialNote>This party may transfer the contract to another party without reference to the issuer, for example by selling it in some marketplace.</skos:editorialNote>
      <rdfs:subClassOf rdf:resource="http://www.omg.org/spec/EDMC-SR/FND/OwnershipAndControl/Ownership/Owner"/>
      <rdfs:subClassOf rdf:resource="http://www.omg.org/spec/EDMC-SR/FND/Agreements/Contracts/ContractCounterparty"/>
   </owl:Class>

   <owl:Class rdf:about="http://www.omg.org/spec/EDMC-SR/FND/Agreements/Contracts/BilateralContract">
      <rdfs:label>Bilateral Contract</rdfs:label>
      <skos:definition>A contract between two specific named parties. The rights and obligations pertaining to either party cannot be transferred to another party without prior written permission or a change to the contract itself.</skos:definition>
      <rdfs:subClassOf rdf:resource="http://www.omg.org/spec/EDMC-SR/FND/Agreements/Contracts/Contract"/>
   </owl:Class>

   <owl:Class rdf:about="http://www.omg.org/spec/EDMC-SR/FND/Agreements/Contracts/TransferableContract">
      <rdfs:label>Transferable Contract</rdfs:label>
   </owl:Class>

   <owl:Class rdf:about="http://www.omg.org/spec/EDMC-SR/FND/Agreements/Contracts/VerbalContract">
      <rdfs:label>Verbal Contract</rdfs:label>
   </owl:Class>

   <owl:Class rdf:about="http://www.omg.org/spec/EDMC-SR/FND/Agreements/Contracts/ContractOriginator">
      <rdfs:label>ContractOriginator</rdfs:label>
      <skos:definition>The party which originates the transferable contract and acts as the Principal in that contract.</skos:definition>
      <rdfs:subClassOf rdf:resource="http://www.omg.org/spec/EDMC-SR/FND/Agreements/Contracts/ContractPrincipal"/>
   </owl:Class>

   <owl:Class rdf:about="http://www.omg.org/spec/EDMC-SR/FND/Agreements/Contracts/WrittenContract">
      <rdfs:label>Written Contract</rdfs:label>
      <skos:definition>A formal Contract which is written and signed by both parties thereto.</skos:definition>
   </owl:Class>

   <!--Individuals-->

</rdf:RDF>