<?xml version="1.0" encoding="UTF-8"?>
  
<!DOCTYPE rdf:RDF [
    <!ENTITY fibo-loan-tmp-bor "http://spec.edmcouncil.org/fibo/red/loan/loans-temporal/loan-borrowers-temporal/">
    <!ENTITY fibo-fnd-info-info "http://spec.edmcouncil.org/fibo/red/fnd/information/info-core/">
    <!ENTITY fibo-loan-tmp-apr "http://spec.edmcouncil.org/fibo/red/loan/loans-temporal/loans-appraisal/">
    <!ENTITY fibo-loan-tmp-app "http://spec.edmcouncil.org/fibo/red/loan/loans-temporal/loan-applications-temporal/">
    <!ENTITY fibo-md-tmp-crr "http://spec.edmcouncil.org/fibo/red/md/temporal-core/credit-ratings/">
    <!ENTITY fibo-fnd-tim-tim "http://spec.edmcouncil.org/fibo/red/fnd/date-time/date-time/">
    <!ENTITY fibo-fnd-utl-bt "http://spec.edmcouncil.org/fibo/red/fnd/utilities/business-facing-types/">
    <!ENTITY fibo-fnd-rel-rel "http://spec.edmcouncil.org/fibo/red/fnd/relations/relations/">
    <!ENTITY fibo-be-le-lp "http://spec.edmcouncil.org/fibo/red/be/legal-entities/legal-persons/">
    <!ENTITY fibo-be-le-cb "http://spec.edmcouncil.org/fibo/red/be/legal-entities/corporate-bodies/">
    <!ENTITY fibo-loan-loan-loan "http://spec.edmcouncil.org/fibo/red/loan/loans/loans-general/">
    <!ENTITY fibo-loan-loan-par "http://spec.edmcouncil.org/fibo/red/loan/loans/loans-parties/">
    <!ENTITY fibo-loan-typ-com "http://spec.edmcouncil.org/fibo/red/loan/loan-types/commercial-loans/">
    <!ENTITY fibo-loan-tmp-ph "http://spec.edmcouncil.org/fibo/red/loan/loans-temporal/loan-phases/">
    <!ENTITY fibo-fnd-acc-cur "http://spec.edmcouncil.org/fibo/red/fnd/accounting/currency-amount/">
]>

<rdf:RDF xmlns:xsd="http://www.w3.org/2001/XMLSchema#"
         xmlns:sm="http://www.omg.org/techprocess/ab/SpecificationMetadata/"
         xmlns:xs="http://www.w3.org/2001/XMLSchema"
         xmlns:fibo-fnd-utl-av="http://www.omg.org/spec/EDMC-FIBO/FND/Utilities/AnnotationVocabulary/"
         xmlns:rdf="http://www.w3.org/1999/02/22-rdf-syntax-ns#"
         xmlns:rdfs="http://www.w3.org/2000/01/rdf-schema#"
         xmlns:owl="http://www.w3.org/2002/07/owl#"
         xmlns:skos="http://www.w3.org/2004/02/skos/core#"
         xmlns:dc="http://purl.org/dc/terms/"
         xml:base="http://spec.edmcouncil.org/fibo/red/loan/loans-temporal/loan-borrowers-temporal/">

   <owl:Ontology rdf:about="http://spec.edmcouncil.org/fibo/red/loan/loans-temporal/loan-borrowers-temporal/">
      <owl:imports rdf:resource="http://spec.edmcouncil.org/fibo/red/fnd/information/info-core/"/>
      <owl:imports rdf:resource="http://spec.edmcouncil.org/fibo/red/loan/loans-temporal/loans-appraisal/"/>
      <owl:imports rdf:resource="http://spec.edmcouncil.org/fibo/red/loan/loans-temporal/loan-applications-temporal/"/>
      <owl:imports rdf:resource="http://spec.edmcouncil.org/fibo/red/md/temporal-core/credit-ratings/"/>
      <owl:imports rdf:resource="http://spec.edmcouncil.org/fibo/red/fnd/date-time/date-time/"/>
      <owl:imports rdf:resource="http://spec.edmcouncil.org/fibo/red/fnd/utilities/business-facing-types/"/>
      <owl:imports rdf:resource="http://spec.edmcouncil.org/fibo/red/fnd/relations/relations/"/>
      <owl:imports rdf:resource="http://spec.edmcouncil.org/fibo/red/be/legal-entities/legal-persons/"/>
      <owl:imports rdf:resource="http://spec.edmcouncil.org/fibo/red/be/legal-entities/corporate-bodies/"/>
      <owl:imports rdf:resource="http://spec.edmcouncil.org/fibo/red/loan/loans/loans-general/"/>
      <owl:imports rdf:resource="http://spec.edmcouncil.org/fibo/red/loan/loans/loans-parties/"/>
      <owl:imports rdf:resource="http://spec.edmcouncil.org/fibo/red/loan/loan-types/commercial-loans/"/>
      <owl:imports rdf:resource="http://spec.edmcouncil.org/fibo/red/loan/loans-temporal/loan-phases/"/>
      <owl:imports rdf:resource="http://spec.edmcouncil.org/fibo/red/fnd/accounting/currency-amount/"/>
   </owl:Ontology>


  <!--
    ///////////////////////////////////////////////////////////////////////////////////////
    //
    // Datatypes
    //
    ///////////////////////////////////////////////////////////////////////////////////////
    -->


<rdfs:Datatype rdf:about="&fibo-loan-tmp-bor;EmploymentStatusSelection">
      <skos:definition>Possible employment statuses for adult human beings.</skos:definition>
      <owl:equivalentClass>
         <rdfs:Datatype>
            <owl:oneOf>
               <rdf:Description>
                  <rdf:first rdf:datatype="http://www.w3.org/2001/XMLSchema#string">Employed</rdf:first>
                  <rdf:rest>
                     <rdf:Description>
                        <rdf:first rdf:datatype="http://www.w3.org/2001/XMLSchema#string">Other</rdf:first>
                        <rdf:rest>
                           <rdf:Description>
                              <rdf:first rdf:datatype="http://www.w3.org/2001/XMLSchema#string">Pensioner</rdf:first>
                              <rdf:rest>
                                 <rdf:Description>
                                    <rdf:first rdf:datatype="http://www.w3.org/2001/XMLSchema#string">Unemployed</rdf:first>
                                    <rdf:rest>
                                       <rdf:Description>
                                          <rdf:first rdf:datatype="http://www.w3.org/2001/XMLSchema#string">Self Employed</rdf:first>
                                          <rdf:rest>
                                             <rdf:Description>
                                                <rdf:first rdf:datatype="http://www.w3.org/2001/XMLSchema#string">Student</rdf:first>
                                                <rdf:rest>
                                                   <rdf:Description>
                                                      <rdf:first rdf:datatype="http://www.w3.org/2001/XMLSchema#string">Protected</rdf:first>
                                                      <rdf:rest rdf:resource="http://www.w3.org/1999/02/22-rdf-syntax-ns#nil"/>
                                                   </rdf:Description>
                                                </rdf:rest>
                                             </rdf:Description>
                                          </rdf:rest>
                                       </rdf:Description>
                                    </rdf:rest>
                                 </rdf:Description>
                              </rdf:rest>
                           </rdf:Description>
                        </rdf:rest>
                     </rdf:Description>
                  </rdf:rest>
               </rdf:Description>
            </owl:oneOf>
         </rdfs:Datatype>
      </owl:equivalentClass>
   </rdfs:Datatype>


  <!--
    ///////////////////////////////////////////////////////////////////////////////////////
    //
    // Object Properties
    //
    ///////////////////////////////////////////////////////////////////////////////////////
    -->


<owl:ObjectProperty rdf:about="&fibo-loan-tmp-bor;isAbout">
      <rdfs:label>is about</rdfs:label>
      <rdfs:domain rdf:resource="&fibo-loan-tmp-bor;BorrowerOngoingDatedFacts"/>
      <rdfs:range rdf:resource="&fibo-loan-tmp-ph;DisbursedLoan"/>
   </owl:ObjectProperty>

   <owl:ObjectProperty rdf:about="&fibo-loan-tmp-bor;isAbout.1">
      <rdfs:label>is about</rdfs:label>
      <rdfs:subPropertyOf rdf:resource="&fibo-loan-tmp-bor;isAbout.4"/>
      <rdfs:domain rdf:resource="&fibo-loan-tmp-bor;CorporateLoanBorrowerAssessmentInformation"/>
      <rdfs:range rdf:resource="&fibo-loan-typ-com;CorporateBorrower"/>
   </owl:ObjectProperty>

   <owl:ObjectProperty rdf:about="&fibo-loan-tmp-bor;identity">
      <rdfs:label>identity</rdfs:label>
      <rdfs:subPropertyOf rdf:resource="&fibo-loan-loan-par;identity"/>
      <rdfs:domain rdf:resource="&fibo-loan-typ-com;CorporateBorrower"/>
      <rdfs:range rdf:resource="&fibo-be-le-cb;BodyCorporate"/>
   </owl:ObjectProperty>

   <owl:ObjectProperty rdf:about="&fibo-loan-tmp-bor;annualProfitAndLoss">
      <rdfs:label>annual profit and loss</rdfs:label>
      <skos:definition>Primary borrower underwritten gross income (not rent), as per most recent Profit and Loss posting.</skos:definition>
      <rdfs:domain rdf:resource="&fibo-loan-tmp-bor;CorporateDatedFacts"/>
      <rdfs:range rdf:resource="&fibo-fnd-acc-cur;MoneyAmount"/>
   </owl:ObjectProperty>

   <owl:ObjectProperty rdf:about="&fibo-loan-tmp-bor;isAbout.2">
      <rdfs:label>is about</rdfs:label>
      <rdfs:subPropertyOf rdf:resource="&fibo-loan-tmp-bor;isAbout"/>
      <rdfs:domain rdf:resource="&fibo-loan-tmp-bor;DelinquencyBorrowerFacts"/>
      <rdfs:range rdf:resource="&fibo-loan-tmp-ph;DelinquentLoan"/>
   </owl:ObjectProperty>

   <owl:ObjectProperty rdf:about="&fibo-loan-tmp-bor;borrowerRatingCreditAmount">
      <rdfs:label>borrower rating credit amount</rdfs:label>
      <skos:definition>Undefined PoC SDM Notes: Credit agency rating of Amount&nbsp;of&nbsp;the&nbsp;credit&nbsp;(Holland&nbsp;only) &lt;/p&gt; &lt;p&gt; (AO 35 , RR 31 ) &lt;/p&gt;</skos:definition>
      <rdfs:domain rdf:resource="&fibo-loan-tmp-bor;IndividualPersonCreditRating"/>
      <rdfs:range rdf:resource="&fibo-fnd-acc-cur;MoneyAmount"/>
   </owl:ObjectProperty>

   <owl:ObjectProperty rdf:about="&fibo-loan-tmp-bor;appraisedBy">
      <rdfs:label>appraised by</rdfs:label>
      <rdfs:domain rdf:resource="&fibo-loan-tmp-app;LoanApplicationBorrowerAssessmentInformation"/>
      <rdfs:range rdf:resource="&fibo-loan-tmp-app;LoanAppraiser"/>
   </owl:ObjectProperty>

   <owl:ObjectProperty rdf:about="&fibo-loan-tmp-bor;isAbout.3">
      <rdfs:label>is about</rdfs:label>
      <rdfs:domain rdf:resource="&fibo-loan-tmp-app;LoanApplicationBorrowerAssessmentInformation"/>
      <rdfs:range rdf:resource="&fibo-loan-tmp-app;LoanApplication"/>
   </owl:ObjectProperty>

   <owl:ObjectProperty rdf:about="&fibo-loan-tmp-bor;isAbout.4">
      <rdfs:label>is about</rdfs:label>
      <rdfs:domain rdf:resource="&fibo-loan-tmp-app;LoanApplicationBorrowerAssessmentInformation"/>
      <rdfs:range rdf:resource="&fibo-loan-loan-par;LoanBorrower"/>
   </owl:ObjectProperty>

   <owl:ObjectProperty rdf:about="&fibo-loan-tmp-bor;includes">
      <rdfs:label>includes</rdfs:label>
      <rdfs:subPropertyOf rdf:resource="&fibo-fnd-rel-rel;hasPart"/>
      <rdfs:domain rdf:resource="&fibo-loan-tmp-bor;PersonalDatedFacts"/>
      <rdfs:range rdf:resource="&fibo-loan-tmp-bor;ArrearsPaymentHistory"/>
   </owl:ObjectProperty>

   <owl:ObjectProperty rdf:about="&fibo-loan-tmp-bor;appraisedBy.1">
      <rdfs:label>appraised by</rdfs:label>
      <rdfs:domain rdf:resource="&fibo-loan-tmp-bor;BorrowerOngoingDatedFacts"/>
      <rdfs:range rdf:resource="&fibo-loan-loan-par;LoanServicer"/>
   </owl:ObjectProperty>

   <owl:ObjectProperty rdf:about="&fibo-loan-tmp-bor;grossIncome">
      <rdfs:label>gross income</rdfs:label>
      <skos:definition>Primary borrower underwritten personal gross income (not rent)</skos:definition>
      <rdfs:domain rdf:resource="&fibo-loan-tmp-bor;PersonalDatedFacts"/>
      <rdfs:range rdf:resource="&fibo-fnd-acc-cur;MonetaryAmount"/>
   </owl:ObjectProperty>

   <owl:ObjectProperty rdf:about="&fibo-loan-tmp-bor;residencyPeriod">
      <rdfs:label>residency period</rdfs:label>
      <skos:definition>Period in which borrower is resident of the country - where the loan property is located.</skos:definition>
      <rdfs:domain rdf:resource="&fibo-loan-tmp-bor;PersonalLoanBorrowerAssessmentInformation"/>
      <rdfs:range rdf:resource="&fibo-fnd-tim-tim;Duration"/>
   </owl:ObjectProperty>

   <owl:ObjectProperty rdf:about="&fibo-loan-tmp-bor;issuedBy">
      <rdfs:label>issued by</rdfs:label>
      <rdfs:subPropertyOf rdf:resource="&fibo-md-tmp-crr;issuedBy"/>
      <rdfs:domain rdf:resource="&fibo-loan-tmp-bor;IndividualPersonCreditRating"/>
      <rdfs:range rdf:resource="&fibo-md-tmp-crr;CreditRatingIssuer"/>
   </owl:ObjectProperty>

   <owl:ObjectProperty rdf:about="&fibo-loan-tmp-bor;rates">
      <rdfs:label>rates</rdfs:label>
      <rdfs:subPropertyOf rdf:resource="&fibo-md-tmp-crr;rates.3"/>
      <rdfs:domain rdf:resource="&fibo-loan-tmp-bor;IndividualPersonCreditRating"/>
      <rdfs:range rdf:resource="&fibo-be-le-lp;NaturalPerson"/>
   </owl:ObjectProperty>


  <!--
    ///////////////////////////////////////////////////////////////////////////////////////
    //
    // Data Properties
    //
    ///////////////////////////////////////////////////////////////////////////////////////
    -->


<owl:DatatypeProperty rdf:about="&fibo-loan-tmp-bor;paymentsMissedInPastSixMonths">
      <rdfs:label>payments missed in past six months</rdfs:label>
      <skos:definition>History of payments missed on previous mortgage in the prior 0-6 months (information as at underwriting).</skos:definition>
      <rdfs:range rdf:resource="&fibo-fnd-utl-bt;yesOrNo"/>
   </owl:DatatypeProperty>

   <owl:DatatypeProperty rdf:about="&fibo-loan-tmp-bor;assessmentDate">
      <rdfs:label>assessment date</rdfs:label>
      <skos:definition>Date at which Borrower income, credit quality, verification, first time status etc were last assessed.</skos:definition>
      <rdfs:range rdf:resource="&fibo-fnd-tim-tim;Date"/>
   </owl:DatatypeProperty>

   <owl:DatatypeProperty rdf:about="&fibo-loan-tmp-bor;repossessionHistory">
      <rdfs:label>repossession history</rdfs:label>
      <skos:definition>If yes: Will be more facts to be determined.</skos:definition>
      <rdfs:range rdf:resource="&fibo-fnd-utl-bt;yesOrNo"/>
   </owl:DatatypeProperty>

   <owl:DatatypeProperty rdf:about="&fibo-loan-tmp-bor;dateOfIncorporation">
      <rdfs:label>date of incorporation</rdfs:label>
      <skos:definition>The date of incorporation of the Corporation.</skos:definition>
      <rdfs:range rdf:resource="http://www.w3.org/2001/XMLSchema#date"/>
   </owl:DatatypeProperty>

   <owl:DatatypeProperty rdf:about="&fibo-loan-tmp-bor;borrowerRatingArrearsSelection">
      <rdfs:label>borrower rating arrears selection</rdfs:label>
      <skos:definition>Undefined PoC SDM Notes: BKR 1 - 10 Arrears code &lt;/p&gt; &lt;p&gt; ArrearscodeaccordingtothecodingofBureauKredietRegistratie(Hollandonly) &lt;/p&gt; &lt;p&gt; ( AO 34, RR 30 ) &lt;/p&gt;</skos:definition>
      <rdfs:range rdf:resource="http://www.w3.org/2001/XMLSchema#string"/>
   </owl:DatatypeProperty>

   <owl:DatatypeProperty rdf:about="&fibo-loan-tmp-bor;borrowerRatingCreditSelection">
      <rdfs:label>borrower rating credit selection</rdfs:label>
      <skos:definition>Undefined PoC SDM Notes: BKR 1-10 Credit type &lt;/p&gt; &lt;p&gt; CredittypeaccordingtothecodingofBureauKredietRegistratie(Hollandonly) &lt;/p&gt; &lt;p&gt; (AO 33 - Agency Rating code , RR 29 ) &lt;/p&gt;</skos:definition>
      <rdfs:range rdf:resource="http://www.w3.org/2001/XMLSchema#string"/>
   </owl:DatatypeProperty>

   <owl:DatatypeProperty rdf:about="&fibo-loan-tmp-bor;borrowerRatingCuredDate">
      <rdfs:label>borrower rating cured date</rdfs:label>
      <skos:definition>Undefined PoC SDM Notes: Is the coding with BKR cured? (Holland only) &lt;/p&gt; &lt;p&gt; If the coding is cured, number of months since it is cured (Holland only) &lt;/p&gt; &lt;p&gt; Represented as a non dirty date if cured &lt;/p&gt;&lt;br /&gt; &lt;p&gt; ( AO 36-37, RR 32- 33 )&nbsp; year month date &lt;/p&gt;</skos:definition>
      <rdfs:range rdf:resource="http://www.w3.org/2001/XMLSchema#date"/>
   </owl:DatatypeProperty>

   <owl:DatatypeProperty rdf:about="&fibo-loan-tmp-bor;borrowerRatingDate">
      <rdfs:label>borrower rating date</rdfs:label>
      <skos:definition>Undefined PoC SDM Notes: The&nbsp;date&nbsp;of&nbsp;the&nbsp;bureau&nbsp;score&nbsp;for&nbsp;this&nbsp;borrower &lt;/p&gt; &lt;p&gt; (AO 40. RR 36 ) &lt;/p&gt;</skos:definition>
      <rdfs:range rdf:resource="http://www.w3.org/2001/XMLSchema#date"/>
   </owl:DatatypeProperty>

   <owl:DatatypeProperty rdf:about="&fibo-loan-tmp-bor;borrowerRatingScoreSelection">
      <rdfs:label>borrower rating score selection</rdfs:label>
      <skos:definition>Undefined PoC SDM Notes: Bureau Score Value - Borrower's Score. &lt;/p&gt; &lt;p&gt; &gt;0 Regular Score&lt;br /&gt; -999 CAIS for mortgage not available&lt;br /&gt; -998 Notice of Correction or Notice of Dispute&lt;br /&gt; 0 Bankruptcy Restriction Order or Bankruptcy Restriction Undertaking &lt;/p&gt; &lt;p&gt; (AO 41, RR 37 ) &lt;/p&gt;</skos:definition>
      <rdfs:range rdf:resource="http://www.w3.org/2001/XMLSchema#string"/>
   </owl:DatatypeProperty>

   <owl:DatatypeProperty rdf:about="&fibo-loan-tmp-bor;borrowerRatingScoreTypeSelection">
      <rdfs:label>borrower rating score type selection</rdfs:label>
      <skos:definition>Undefined PoC SDM Notes: This is partially expressed by party id of the issuing agency &lt;/p&gt; &lt;p&gt; But some of these scores are also methods ( internal / Other ) &lt;/p&gt; &lt;p&gt; Who has provided the score. For continental Europe give name of provider. &lt;/p&gt; &lt;p&gt; Callcredit (1)&lt;br /&gt; Experian (2)&lt;br /&gt; Equifax (3)&lt;br /&gt; Schufa (4)&lt;br /&gt; BKR (5)&lt;br /&gt; Internal Score (6)&lt;br /&gt; Other (7) &lt;/p&gt; &lt;p&gt; ( AO 38 - originally Party id , RR 34 )&lt;br /&gt; No data (ND) &lt;/p&gt;</skos:definition>
      <rdfs:range rdf:resource="http://www.w3.org/2001/XMLSchema#string"/>
   </owl:DatatypeProperty>

   <owl:DatatypeProperty rdf:about="&fibo-loan-tmp-bor;borrowerRatingTypeSelection">
      <rdfs:label>borrower rating type selection</rdfs:label>
      <skos:definition>Undefined PoC SDM Notes: Bureau Score Type - Type of scorecard provided. &lt;/p&gt; &lt;p&gt; Generation 8 B&amp;F AAM - DCM (Experian) (1)&lt;br /&gt; Generation 8 B&amp;F CRS - DCM (Experian) (2)&lt;br /&gt; Generation 7 Mortgage PD Score - DCM (Experian) (3)&lt;br /&gt; FSC109 - Risk Navigator (Equifax) (4)&lt;br /&gt; RNILF02 - Risk Navigator (Equifax) (5)&lt;br /&gt; RNISF02 - Risk Navigator (Equifax) (6)&lt;br /&gt; Internal Scorecard (7)&lt;br /&gt; Other (provide details) (8)&lt;br /&gt; No data (ND) &lt;/p&gt; &lt;p&gt; ( AO 39, RR 35 ) &lt;/p&gt;</skos:definition>
      <rdfs:range rdf:resource="http://www.w3.org/2001/XMLSchema#string"/>
   </owl:DatatypeProperty>

   <owl:DatatypeProperty rdf:about="&fibo-loan-tmp-bor;employmentStatus">
      <rdfs:label>employment status</rdfs:label>
      <skos:definition>Employment Status; Employment status of (the primary) applicant.</skos:definition>
      <rdfs:range rdf:resource="&fibo-loan-tmp-bor;EmploymentStatusSelection"/>
   </owl:DatatypeProperty>

   <owl:DatatypeProperty rdf:about="&fibo-loan-tmp-bor;history1-6MArrearsPayments">
      <rdfs:label>history 1-6 m arrears payments</rdfs:label>
      <skos:definition>History - use timed status values and timed status information entity which has present and past values.</skos:definition>
   </owl:DatatypeProperty>

   <owl:DatatypeProperty rdf:about="&fibo-loan-tmp-bor;history6+MArrearsPayments">
      <rdfs:label>history 6+ m arrears payments</rdfs:label>
      <skos:definition>As above History&nbsp;of payments missed on previous mortgage(s) with months &gt; 6M in arrears&nbsp; &lt;/p&gt; &lt;p&gt; RR has&nbsp;count of payments missed - but&nbsp; the form here with associated dates will mean that enterered data remains valid over time dirty data &lt;/p&gt; &lt;p&gt; History of (non)payments&nbsp;6+ months in arrears on preceding mortgages &lt;/p&gt; &lt;p&gt; Data form is a list with dates and indicated event ( OK / arrears&nbsp; 6+ Mo ) &lt;/p&gt; &lt;p&gt; (AO 24, RR 40 ) &nbsp; &lt;/p&gt;</skos:definition>
   </owl:DatatypeProperty>

   <owl:DatatypeProperty rdf:about="&fibo-loan-tmp-bor;reposessionHistory">
      <rdfs:label>reposession history</rdfs:label>
      <skos:definition>Whether there is a hirstory of prior repossessions resulting from the borrower defaulting on a previous mortgage loan.</skos:definition>
      <rdfs:range rdf:resource="&fibo-fnd-utl-bt;yesOrNo"/>
   </owl:DatatypeProperty>

   <owl:DatatypeProperty rdf:about="&fibo-loan-tmp-bor;employmentStatus.1">
      <rdfs:label>employment status</rdfs:label>
      <skos:definition>The employment status of the person applying for the loan, e.g. employed, self-employed, unemployed.</skos:definition>
      <rdfs:range rdf:resource="&fibo-loan-tmp-bor;EmploymentStatusSelection"/>
   </owl:DatatypeProperty>

   <owl:DatatypeProperty rdf:about="&fibo-loan-tmp-bor;incomeVerificationMethod">
      <rdfs:label>income verification method</rdfs:label>
      <skos:definition>Income verification method for borrowers income.</skos:definition>
      <rdfs:range rdf:resource="&fibo-loan-loan-loan;IncomeVerificationMethodSelection"/>
   </owl:DatatypeProperty>

   <owl:DatatypeProperty rdf:about="&fibo-loan-tmp-bor;referenceContactInformation">
      <rdfs:label>reference contact information</rdfs:label>
      <skos:definition>contact information on file for the references taken up on the potential borrower(s).</skos:definition>
      <rdfs:range rdf:resource="&fibo-fnd-utl-bt;text"/>
   </owl:DatatypeProperty>


  <!--
    ///////////////////////////////////////////////////////////////////////////////////////
    //
    // Annotation Properties
    //
    ///////////////////////////////////////////////////////////////////////////////////////
    -->



  <!--
    ///////////////////////////////////////////////////////////////////////////////////////
    //
    // Classes
    //
    ///////////////////////////////////////////////////////////////////////////////////////
    -->


<owl:Class rdf:about="&fibo-loan-tmp-bor;ArrearsPaymentHistory">
      <rdfs:label>arrears payment history</rdfs:label>
      <skos:definition>Historical information about payment of arrears by the entity.</skos:definition>
   </owl:Class>

   <owl:Class rdf:about="&fibo-loan-tmp-bor;BorrowerOngoingDatedFacts">
      <rdfs:label>borrower ongoing dated facts</rdfs:label>
      <skos:definition>Ongoing information about the borrower.</skos:definition>
   </owl:Class>

   <owl:Class rdf:about="&fibo-loan-tmp-bor;CorporateDatedFacts">
      <rdfs:label>corporate dated facts</rdfs:label>
      <rdfs:subClassOf rdf:resource="&fibo-loan-tmp-bor;BorrowerOngoingDatedFacts"/>
   </owl:Class>

   <owl:Class rdf:about="&fibo-loan-tmp-bor;CorporateLoanBorrowerAssessmentInformation">
      <rdfs:label>corporate loan borrower assessment information</rdfs:label>
      <rdfs:subClassOf rdf:resource="&fibo-loan-tmp-app;LoanApplicationBorrowerAssessmentInformation"/>
   </owl:Class>

   <owl:Class rdf:about="&fibo-loan-tmp-bor;DelinquencyBorrowerFacts">
      <rdfs:label>delinquency borrower facts</rdfs:label>
      <skos:definition>Facts about the borroewr in the event of some delinquency.</skos:definition>
   </owl:Class>

   <owl:Class rdf:about="&fibo-loan-tmp-bor;IndividualPersonCreditRating">
      <rdfs:label>individual person credit rating</rdfs:label>
      <skos:definition>was Borrower Credit Rating</skos:definition>
      <rdfs:subClassOf rdf:resource="&fibo-md-tmp-crr;IndividualCreditRating"/>
   </owl:Class>

   <owl:Class rdf:about="&fibo-loan-tmp-bor;PersonalAssessmentFactsAtApproval">
      <rdfs:label>personal assessment facts at approval</rdfs:label>
      <skos:definition>Pertinent economic facts about an individual person at the time a given loan was approved.</skos:definition>
      <rdfs:subClassOf rdf:resource="&fibo-loan-tmp-bor;PersonalDatedFacts"/>
   </owl:Class>

   <owl:Class rdf:about="&fibo-loan-tmp-bor;PersonalDatedFacts">
      <rdfs:label>personal dated facts</rdfs:label>
      <skos:definition>Facts about a natural person. These are facts that are true as at a given time.</skos:definition>
      <rdfs:subClassOf rdf:resource="&fibo-fnd-info-info;Information"/>
   </owl:Class>

   <owl:Class rdf:about="&fibo-loan-tmp-bor;PersonalLoanBorrowerAssessmentInformation">
      <rdfs:label>personal loan borrower assessment information</rdfs:label>
   </owl:Class>

   <owl:Class rdf:about="&fibo-loan-tmp-bor;PersonalMortgageLoanBorrowerAssessmentInformation">
      <rdfs:label>personal mortgage loan borrower assessment information</rdfs:label>
      <rdfs:subClassOf rdf:resource="&fibo-loan-tmp-apr;MortgageLoanBorrowerAssessmentInformation"/>
      <rdfs:subClassOf rdf:resource="&fibo-loan-tmp-bor;PersonalLoanBorrowerAssessmentInformation"/>
   </owl:Class>


  <!--
    ///////////////////////////////////////////////////////////////////////////////////////
    //
    // Individuals
    //
    ///////////////////////////////////////////////////////////////////////////////////////
    -->


</rdf:RDF>