<?xml version="1.0" encoding="UTF-8"?>
<!DOCTYPE rdf:RDF [
	<!ENTITY dct "http://purl.org/dc/terms/">
	<!ENTITY fibo-be-ge-ge "https://spec.edmcouncil.org/fibo/ontology/BE/GovernmentEntities/GovernmentEntities/">
	<!ENTITY fibo-be-ge-usj "https://spec.edmcouncil.org/fibo/ontology/BE/GovernmentEntities/NorthAmericanJurisdiction/USGovernmentEntitiesAndJurisdictions/">
	<!ENTITY fibo-fbc-fct-breg "https://spec.edmcouncil.org/fibo/ontology/FBC/FunctionalEntities/BusinessRegistries/">
	<!ENTITY fibo-fbc-fct-ra "https://spec.edmcouncil.org/fibo/ontology/FBC/FunctionalEntities/RegistrationAuthorities/">
	<!ENTITY fibo-fbc-fct-rga "https://spec.edmcouncil.org/fibo/ontology/FBC/FunctionalEntities/RegulatoryAgencies/">
	<!ENTITY fibo-fbc-fct-uspsaa "https://spec.edmcouncil.org/fibo/ontology/FBC/FunctionalEntities/NorthAmericanEntities/USPostalServiceAndAddressing/">
	<!ENTITY fibo-fnd-aap-agt "https://spec.edmcouncil.org/fibo/ontology/FND/AgentsAndPeople/Agents/">
	<!ENTITY fibo-fnd-arr-arr "https://spec.edmcouncil.org/fibo/ontology/FND/Arrangements/Arrangements/">
	<!ENTITY fibo-fnd-arr-cd "https://spec.edmcouncil.org/fibo/ontology/FND/Arrangements/Codes/">
	<!ENTITY fibo-fnd-arr-cls "https://spec.edmcouncil.org/fibo/ontology/FND/Arrangements/ClassificationSchemes/">
	<!ENTITY fibo-fnd-arr-id "https://spec.edmcouncil.org/fibo/ontology/FND/Arrangements/IdentifiersAndIndices/">
	<!ENTITY fibo-fnd-plc-adr "https://spec.edmcouncil.org/fibo/ontology/FND/Places/Addresses/">
	<!ENTITY fibo-fnd-plc-cty "https://spec.edmcouncil.org/fibo/ontology/FND/Places/Countries/">
	<!ENTITY fibo-fnd-rel-rel "https://spec.edmcouncil.org/fibo/ontology/FND/Relations/Relations/">
	<!ENTITY fibo-fnd-utl-av "https://spec.edmcouncil.org/fibo/ontology/FND/Utilities/AnnotationVocabulary/">
	<!ENTITY lcc-3166-1 "https://www.omg.org/spec/LCC/Countries/ISO3166-1-CountryCodes/">
	<!ENTITY lcc-cr "https://www.omg.org/spec/LCC/Countries/CountryRepresentation/">
	<!ENTITY lcc-lr "https://www.omg.org/spec/LCC/Languages/LanguageRepresentation/">
	<!ENTITY owl "http://www.w3.org/2002/07/owl#">
	<!ENTITY rdf "http://www.w3.org/1999/02/22-rdf-syntax-ns#">
	<!ENTITY rdfs "http://www.w3.org/2000/01/rdf-schema#">
	<!ENTITY skos "http://www.w3.org/2004/02/skos/core#">
	<!ENTITY sm "http://www.omg.org/techprocess/ab/SpecificationMetadata/">
	<!ENTITY xsd "http://www.w3.org/2001/XMLSchema#">
]>
<rdf:RDF xml:base="https://spec.edmcouncil.org/fibo/ontology/FBC/FunctionalEntities/NorthAmericanEntities/USPostalServiceAndAddressing/"
	xmlns:dct="http://purl.org/dc/terms/"
	xmlns:fibo-be-ge-ge="https://spec.edmcouncil.org/fibo/ontology/BE/GovernmentEntities/GovernmentEntities/"
	xmlns:fibo-be-ge-usj="https://spec.edmcouncil.org/fibo/ontology/BE/GovernmentEntities/NorthAmericanJurisdiction/USGovernmentEntitiesAndJurisdictions/"
	xmlns:fibo-fbc-fct-breg="https://spec.edmcouncil.org/fibo/ontology/FBC/FunctionalEntities/BusinessRegistries/"
	xmlns:fibo-fbc-fct-ra="https://spec.edmcouncil.org/fibo/ontology/FBC/FunctionalEntities/RegistrationAuthorities/"
	xmlns:fibo-fbc-fct-rga="https://spec.edmcouncil.org/fibo/ontology/FBC/FunctionalEntities/RegulatoryAgencies/"
	xmlns:fibo-fbc-fct-uspsaa="https://spec.edmcouncil.org/fibo/ontology/FBC/FunctionalEntities/NorthAmericanEntities/USPostalServiceAndAddressing/"
	xmlns:fibo-fnd-aap-agt="https://spec.edmcouncil.org/fibo/ontology/FND/AgentsAndPeople/Agents/"
	xmlns:fibo-fnd-arr-arr="https://spec.edmcouncil.org/fibo/ontology/FND/Arrangements/Arrangements/"
	xmlns:fibo-fnd-arr-cd="https://spec.edmcouncil.org/fibo/ontology/FND/Arrangements/Codes/"
	xmlns:fibo-fnd-arr-cls="https://spec.edmcouncil.org/fibo/ontology/FND/Arrangements/ClassificationSchemes/"
	xmlns:fibo-fnd-arr-id="https://spec.edmcouncil.org/fibo/ontology/FND/Arrangements/IdentifiersAndIndices/"
	xmlns:fibo-fnd-plc-adr="https://spec.edmcouncil.org/fibo/ontology/FND/Places/Addresses/"
	xmlns:fibo-fnd-plc-cty="https://spec.edmcouncil.org/fibo/ontology/FND/Places/Countries/"
	xmlns:fibo-fnd-rel-rel="https://spec.edmcouncil.org/fibo/ontology/FND/Relations/Relations/"
	xmlns:fibo-fnd-utl-av="https://spec.edmcouncil.org/fibo/ontology/FND/Utilities/AnnotationVocabulary/"
	xmlns:lcc-3166-1="https://www.omg.org/spec/LCC/Countries/ISO3166-1-CountryCodes/"
	xmlns:lcc-cr="https://www.omg.org/spec/LCC/Countries/CountryRepresentation/"
	xmlns:lcc-lr="https://www.omg.org/spec/LCC/Languages/LanguageRepresentation/"
	xmlns:owl="http://www.w3.org/2002/07/owl#"
	xmlns:rdf="http://www.w3.org/1999/02/22-rdf-syntax-ns#"
	xmlns:rdfs="http://www.w3.org/2000/01/rdf-schema#"
	xmlns:skos="http://www.w3.org/2004/02/skos/core#"
	xmlns:sm="http://www.omg.org/techprocess/ab/SpecificationMetadata/"
	xmlns:xsd="http://www.w3.org/2001/XMLSchema#">
	
	<owl:Ontology rdf:about="https://spec.edmcouncil.org/fibo/ontology/FBC/FunctionalEntities/NorthAmericanEntities/USPostalServiceAndAddressing/">
		<rdfs:label>U.S. Postal Service and Addressing Ontology</rdfs:label>
		<dct:abstract>This ontology augments others in FBC that define US government and regulatory agencies with individuals representing the U.S. Postal Service as well as address concepts that conform to the USPS Pub 28.  The USPS provides automated address verification services that use the concepts defined herein for that purpose, and which many financial services entities use for data quality purposes.</dct:abstract>
		<dct:license rdf:datatype="&xsd;anyURI">http://opensource.org/licenses/MIT</dct:license>
		<sm:contentLanguage rdf:datatype="&xsd;anyURI">http://www.w3.org/standards/techs/owl#w3c_all</sm:contentLanguage>
		<sm:copyright>Copyright (c) 2019 EDM Council, Inc.</sm:copyright>
		<sm:dependsOn rdf:datatype="&xsd;anyURI">https://spec.edmcouncil.org/fibo/ontology/BE/</sm:dependsOn>
		<sm:dependsOn rdf:datatype="&xsd;anyURI">https://spec.edmcouncil.org/fibo/ontology/FBC/FunctionalEntities/BusinessRegistries/</sm:dependsOn>
		<sm:dependsOn rdf:datatype="&xsd;anyURI">https://spec.edmcouncil.org/fibo/ontology/FBC/FunctionalEntities/RegistrationAuthorities/</sm:dependsOn>
		<sm:dependsOn rdf:datatype="&xsd;anyURI">https://spec.edmcouncil.org/fibo/ontology/FBC/FunctionalEntities/RegulatoryAgencies/</sm:dependsOn>
		<sm:dependsOn rdf:datatype="&xsd;anyURI">https://spec.edmcouncil.org/fibo/ontology/FND/</sm:dependsOn>
		<sm:fileAbbreviation>fibo-fbc-fct-uspsaa</sm:fileAbbreviation>
		<sm:filename>USPostalServiceAndAddressing.rdf</sm:filename>
		<rdfs:seeAlso rdf:resource="https://about.usps.com/who/profile/"/>
		<rdfs:seeAlso rdf:resource="https://pe.usps.com/cpim/ftp/pubs/Pub28/pub28.pdf"/>
		<owl:imports rdf:resource="https://spec.edmcouncil.org/fibo/ontology/BE/GovernmentEntities/GovernmentEntities/"/>
		<owl:imports rdf:resource="https://spec.edmcouncil.org/fibo/ontology/BE/GovernmentEntities/NorthAmericanJurisdiction/USGovernmentEntitiesAndJurisdictions/"/>
		<owl:imports rdf:resource="https://spec.edmcouncil.org/fibo/ontology/FBC/FunctionalEntities/BusinessRegistries/"/>
		<owl:imports rdf:resource="https://spec.edmcouncil.org/fibo/ontology/FBC/FunctionalEntities/RegistrationAuthorities/"/>
		<owl:imports rdf:resource="https://spec.edmcouncil.org/fibo/ontology/FBC/FunctionalEntities/RegulatoryAgencies/"/>
		<owl:imports rdf:resource="https://spec.edmcouncil.org/fibo/ontology/FND/AgentsAndPeople/Agents/"/>
		<owl:imports rdf:resource="https://spec.edmcouncil.org/fibo/ontology/FND/Arrangements/Arrangements/"/>
		<owl:imports rdf:resource="https://spec.edmcouncil.org/fibo/ontology/FND/Arrangements/ClassificationSchemes/"/>
		<owl:imports rdf:resource="https://spec.edmcouncil.org/fibo/ontology/FND/Arrangements/Codes/"/>
		<owl:imports rdf:resource="https://spec.edmcouncil.org/fibo/ontology/FND/Arrangements/IdentifiersAndIndices/"/>
		<owl:imports rdf:resource="https://spec.edmcouncil.org/fibo/ontology/FND/Places/Addresses/"/>
		<owl:imports rdf:resource="https://spec.edmcouncil.org/fibo/ontology/FND/Places/Countries/"/>
		<owl:imports rdf:resource="https://spec.edmcouncil.org/fibo/ontology/FND/Relations/Relations/"/>
		<owl:imports rdf:resource="https://spec.edmcouncil.org/fibo/ontology/FND/Utilities/AnnotationVocabulary/"/>
		<owl:imports rdf:resource="https://www.omg.org/spec/LCC/Countries/CountryRepresentation/"/>
		<owl:imports rdf:resource="https://www.omg.org/spec/LCC/Countries/ISO3166-1-CountryCodes/"/>
		<owl:imports rdf:resource="https://www.omg.org/spec/LCC/Languages/LanguageRepresentation/"/>
		<owl:versionIRI rdf:resource="https://spec.edmcouncil.org/fibo/ontology/FBC/20190701/FunctionalEntities/NorthAmericanEntities/USPostalServiceAndAddressing/"/>
		<fibo-fnd-utl-av:hasMaturityLevel rdf:resource="&fibo-fnd-utl-av;Release"/>
	</owl:Ontology>
	
	<owl:Class rdf:about="&fibo-fbc-fct-uspsaa;AddressComponent">
		<rdfs:subClassOf rdf:resource="&fibo-fnd-arr-id;Index"/>
		<rdfs:label>address component</rdfs:label>
		<skos:definition>part of a delivery address that is an index in its own right</skos:definition>
	</owl:Class>
	
	<owl:Class rdf:about="&fibo-fbc-fct-uspsaa;CompleteAddress">
		<rdfs:subClassOf rdf:resource="&fibo-fbc-fct-uspsaa;StandardizedAddress"/>
		<rdfs:label>complete address</rdfs:label>
		<skos:definition>delivery address that has all the address elements necessary to allow an exact match with the current Postal Service ZIP+4 and City State files to obtain the finest level of ZIP+4 and delivery point codes for the delivery address</skos:definition>
		<fibo-fnd-utl-av:explanatoryNote>A complete address may be required on mail at some automation rates.</fibo-fnd-utl-av:explanatoryNote>
	</owl:Class>
	
	<owl:Class rdf:about="&fibo-fbc-fct-uspsaa;ConventionalDeliveryAddress">
		<rdfs:subClassOf rdf:resource="&fibo-fbc-fct-uspsaa;DeliveryAddress"/>
		<rdfs:subClassOf>
			<owl:Restriction>
				<owl:onProperty rdf:resource="&fibo-fnd-arr-arr;hasConstituent"/>
				<owl:onClass rdf:resource="&fibo-fbc-fct-uspsaa;StreetAddress"/>
				<owl:qualifiedCardinality rdf:datatype="&xsd;nonNegativeInteger">1</owl:qualifiedCardinality>
			</owl:Restriction>
		</rdfs:subClassOf>
		<rdfs:label>conventional delivery address</rdfs:label>
		<skos:definition>delivery address that includes a street address</skos:definition>
	</owl:Class>
	
	<owl:Class rdf:about="&fibo-fbc-fct-uspsaa;DeliveryAddress">
		<rdfs:subClassOf rdf:resource="&fibo-fnd-plc-adr;PhysicalAddress"/>
		<rdfs:subClassOf>
			<owl:Class>
				<owl:unionOf rdf:parseType="Collection">
					<owl:Restriction>
						<owl:onProperty rdf:resource="&fibo-fbc-fct-breg;hasCity"/>
						<owl:onDataRange rdf:resource="&rdfs;Literal"/>
						<owl:qualifiedCardinality rdf:datatype="&xsd;nonNegativeInteger">1</owl:qualifiedCardinality>
					</owl:Restriction>
					<owl:Restriction>
						<owl:onProperty rdf:resource="&fibo-fbc-fct-breg;hasMunicipality"/>
						<owl:onClass rdf:resource="&fibo-fnd-plc-cty;Municipality"/>
						<owl:qualifiedCardinality rdf:datatype="&xsd;nonNegativeInteger">1</owl:qualifiedCardinality>
					</owl:Restriction>
				</owl:unionOf>
			</owl:Class>
		</rdfs:subClassOf>
		<rdfs:subClassOf>
			<owl:Restriction>
				<owl:onProperty rdf:resource="&fibo-fnd-rel-rel;isDefinedIn"/>
				<owl:onClass rdf:resource="&fibo-fbc-fct-uspsaa;DeliveryAddressingScheme"/>
				<owl:qualifiedCardinality rdf:datatype="&xsd;nonNegativeInteger">1</owl:qualifiedCardinality>
			</owl:Restriction>
		</rdfs:subClassOf>
		<rdfs:subClassOf>
			<owl:Restriction>
				<owl:onProperty rdf:resource="&fibo-fbc-fct-uspsaa;hasPostcode"/>
				<owl:onClass rdf:resource="&fibo-fbc-fct-uspsaa;Postcode"/>
				<owl:qualifiedCardinality rdf:datatype="&xsd;nonNegativeInteger">1</owl:qualifiedCardinality>
			</owl:Restriction>
		</rdfs:subClassOf>
		<rdfs:subClassOf>
			<owl:Restriction>
				<owl:onProperty rdf:resource="&fibo-fbc-fct-breg;hasSubdivision"/>
				<owl:someValuesFrom rdf:resource="&lcc-cr;CountrySubdivision"/>
			</owl:Restriction>
		</rdfs:subClassOf>
		<rdfs:label>delivery address</rdfs:label>
		<skos:definition>location (destination) to which something may be delivered</skos:definition>
		<fibo-fnd-utl-av:explanatoryNote>In the United States, a delivery address is a postal address conforming with United States Postal Service (USPS) addressing requirements specified in Publication 28 - Postal Addressing Standards.  Every U.S. Publication 28 conformant postal address is a physical delivery address, although certain addresses, such as post office box or general delivery addrsses typically have a public or private post office as their delivery point rather than a residence or business.</fibo-fnd-utl-av:explanatoryNote>
	</owl:Class>
	
	<owl:Class rdf:about="&fibo-fbc-fct-uspsaa;DeliveryAddressCodeSet">
		<rdfs:subClassOf rdf:resource="&fibo-fnd-arr-cd;CodeSet"/>
		<rdfs:subClassOf rdf:resource="&fibo-fnd-arr-id;IdentificationScheme"/>
		<rdfs:subClassOf>
			<owl:Restriction>
				<owl:onProperty rdf:resource="&fibo-fnd-rel-rel;hasMember"/>
				<owl:someValuesFrom rdf:resource="&fibo-fbc-fct-uspsaa;DeliveryAddressIdentifier"/>
			</owl:Restriction>
		</rdfs:subClassOf>
		<rdfs:label>delivery point code set</rdfs:label>
		<rdfs:seeAlso rdf:resource="https://pe.usps.com/cpim/ftp/pubs/Pub28/pub28.pdf"/>
		<skos:definition>system of numeric codes that substitute for specified delivery point details according to the U.S. Postal Service Publication 28</skos:definition>
	</owl:Class>
	
	<owl:Class rdf:about="&fibo-fbc-fct-uspsaa;DeliveryAddressIdentifier">
		<rdfs:subClassOf rdf:resource="&fibo-fnd-arr-cd;CodeElement"/>
		<rdfs:subClassOf rdf:resource="&fibo-fnd-arr-id;Identifier"/>
		<rdfs:subClassOf>
			<owl:Restriction>
				<owl:onProperty rdf:resource="&fibo-fnd-aap-agt;identifies"/>
				<owl:onClass rdf:resource="&fibo-fbc-fct-uspsaa;DeliveryAddress"/>
				<owl:qualifiedCardinality rdf:datatype="&xsd;nonNegativeInteger">1</owl:qualifiedCardinality>
			</owl:Restriction>
		</rdfs:subClassOf>
		<rdfs:subClassOf>
			<owl:Restriction>
				<owl:onProperty rdf:resource="&fibo-fnd-rel-rel;isDefinedIn"/>
				<owl:onClass rdf:resource="&fibo-fbc-fct-uspsaa;DeliveryAddressingScheme"/>
				<owl:qualifiedCardinality rdf:datatype="&xsd;nonNegativeInteger">1</owl:qualifiedCardinality>
			</owl:Restriction>
		</rdfs:subClassOf>
		<rdfs:subClassOf>
			<owl:Restriction>
				<owl:onProperty rdf:resource="&fibo-fnd-arr-arr;hasConstituent"/>
				<owl:onClass rdf:resource="&fibo-fbc-fct-uspsaa;DeliveryPointCode"/>
				<owl:qualifiedCardinality rdf:datatype="&xsd;nonNegativeInteger">1</owl:qualifiedCardinality>
			</owl:Restriction>
		</rdfs:subClassOf>
		<rdfs:subClassOf>
			<owl:Restriction>
				<owl:onProperty rdf:resource="&fibo-fnd-arr-arr;hasConstituent"/>
				<owl:onClass rdf:resource="&fibo-fbc-fct-uspsaa;ZIPPlus4Code"/>
				<owl:qualifiedCardinality rdf:datatype="&xsd;nonNegativeInteger">1</owl:qualifiedCardinality>
			</owl:Restriction>
		</rdfs:subClassOf>
		<rdfs:label>delivery address identifier</rdfs:label>
		<skos:definition></skos:definition>
		<skos:definition>unique identifier for a location (destination) to which something is delivered</skos:definition>
		<fibo-fnd-utl-av:explanatoryNote>When combined with the ZIP + 4 code, the delivery point code provides a unique identifier for every deliverable address served by the USPS.  The delivery point digits are almost never printed on mail in human-readable form; instead they are encoded in the POSTNET delivery point barcode (DPBC) or as part of the newer Intelligent Mail Barcode (IMB).</fibo-fnd-utl-av:explanatoryNote>
	</owl:Class>
	
	<owl:Class rdf:about="&fibo-fbc-fct-uspsaa;DeliveryAddressingScheme">
		<rdfs:subClassOf rdf:resource="&fibo-fnd-plc-adr;AddressingScheme"/>
		<rdfs:subClassOf>
			<owl:Restriction>
				<owl:onProperty rdf:resource="&fibo-fnd-rel-rel;defines"/>
				<owl:someValuesFrom rdf:resource="&fibo-fbc-fct-uspsaa;DeliveryAddress"/>
			</owl:Restriction>
		</rdfs:subClassOf>
		<rdfs:label>delivery addressing scheme</rdfs:label>
		<rdfs:seeAlso rdf:resource="https://pe.usps.com/cpim/ftp/pubs/Pub28/pub28.pdf"/>
		<skos:definition>scheme for defining delivery addresses according to the U.S. Postal Service Publication 28</skos:definition>
	</owl:Class>
	
	<owl:Class rdf:about="&fibo-fbc-fct-uspsaa;DeliveryPointCode">
		<rdfs:subClassOf rdf:resource="&fibo-fnd-arr-cd;CodeElement"/>
		<rdfs:subClassOf>
			<owl:Restriction>
				<owl:onProperty rdf:resource="&fibo-fnd-rel-rel;isMemberOf"/>
				<owl:onClass rdf:resource="&fibo-fbc-fct-uspsaa;DeliveryPointCodeSet"/>
				<owl:qualifiedCardinality rdf:datatype="&xsd;nonNegativeInteger">1</owl:qualifiedCardinality>
			</owl:Restriction>
		</rdfs:subClassOf>
		<rdfs:subClassOf>
			<owl:Restriction>
				<owl:onProperty rdf:resource="&fibo-fnd-rel-rel;hasTag"/>
				<owl:onDataRange rdf:resource="&xsd;string"/>
				<owl:qualifiedCardinality rdf:datatype="&xsd;nonNegativeInteger">1</owl:qualifiedCardinality>
			</owl:Restriction>
		</rdfs:subClassOf>
		<rdfs:label>delivery point code</rdfs:label>
		<rdfs:seeAlso rdf:resource="https://pe.usps.com/cpim/ftp/pubs/Pub28/pub28.pdf"/>
		<skos:definition>specific set of digits between 00 and 99 assigned to a delivery point</skos:definition>
		<fibo-fnd-utl-av:explanatoryNote>When combined with the ZIP + 4 code, the delivery point code provides a unique identifier for every deliverable address served by the USPS.  The delivery point digits are almost never printed on mail in human-readable form; instead they are encoded in the POSTNET delivery point barcode (DPBC) or as part of the newer Intelligent Mail Barcode (IMB).</fibo-fnd-utl-av:explanatoryNote>
	</owl:Class>
	
	<owl:Class rdf:about="&fibo-fbc-fct-uspsaa;DeliveryPointCodeSet">
		<rdfs:subClassOf rdf:resource="&fibo-fnd-arr-cd;CodeSet"/>
		<rdfs:subClassOf>
			<owl:Restriction>
				<owl:onProperty rdf:resource="&fibo-fnd-rel-rel;hasMember"/>
				<owl:someValuesFrom rdf:resource="&fibo-fbc-fct-uspsaa;DeliveryPointCode"/>
			</owl:Restriction>
		</rdfs:subClassOf>
		<rdfs:label>delivery point code set</rdfs:label>
		<rdfs:seeAlso rdf:resource="https://pe.usps.com/cpim/ftp/pubs/Pub28/pub28.pdf"/>
		<skos:definition>system of numeric codes that substitute for specified delivery point details according to the U.S. Postal Service Publication 28</skos:definition>
	</owl:Class>
	
	<owl:Class rdf:about="&fibo-fbc-fct-uspsaa;DepartmentOfStateAddress">
		<rdfs:subClassOf rdf:resource="&fibo-fbc-fct-uspsaa;DeliveryAddress"/>
		<rdfs:subClassOf>
			<owl:Restriction>
				<owl:onProperty rdf:resource="&fibo-fbc-fct-breg;hasCity"/>
				<owl:hasValue>DPO</owl:hasValue>
			</owl:Restriction>
		</rdfs:subClassOf>
		<rdfs:subClassOf>
			<owl:Restriction>
				<owl:onProperty rdf:resource="&fibo-fbc-fct-breg;hasAddressLine1"/>
				<owl:onDataRange rdf:resource="&rdfs;Literal"/>
				<owl:qualifiedCardinality rdf:datatype="&xsd;nonNegativeInteger">1</owl:qualifiedCardinality>
			</owl:Restriction>
		</rdfs:subClassOf>
		<rdfs:label>Department of State address</rdfs:label>
		<owl:disjointWith rdf:resource="&fibo-fbc-fct-uspsaa;ConventionalDeliveryAddress"/>
		<skos:definition>delivery address whose delivery address line uses &apos;UNIT&apos; followed by the unit identifier, followed by &apos;BOX&apos; followed by box number, in place of a street address, &apos;DPO&apos; as the literal value for the city, and the appropriate armed forces subdivision code in place of a subdivision (state) code</skos:definition>
	</owl:Class>
	
	<owl:NamedIndividual rdf:about="&fibo-fbc-fct-uspsaa;East">
		<rdf:type rdf:resource="&fibo-fbc-fct-uspsaa;GeographicDirectionalSymbol"/>
		<rdfs:label xml:lang="en">East</rdfs:label>
		<rdfs:label xml:lang="es">Este</rdfs:label>
		<skos:definition>geographic directional symbol for East</skos:definition>
		<fibo-fnd-rel-rel:hasTag>E</fibo-fnd-rel-rel:hasTag>
	</owl:NamedIndividual>
	
	<owl:Class rdf:about="&fibo-fbc-fct-uspsaa;GeneralDeliveryAddress">
		<rdfs:subClassOf rdf:resource="&fibo-fbc-fct-uspsaa;DeliveryAddress"/>
		<rdfs:subClassOf>
			<owl:Restriction>
				<owl:onProperty rdf:resource="&fibo-fbc-fct-breg;hasAddressLine1"/>
				<owl:hasValue>GENERAL DELIVERY</owl:hasValue>
			</owl:Restriction>
		</rdfs:subClassOf>
		<rdfs:label>general delivery address</rdfs:label>
		<owl:disjointWith rdf:resource="&fibo-fbc-fct-uspsaa;ConventionalDeliveryAddress"/>
		<skos:definition>delivery address that uses the words &apos;GENERAL DELIVERY&apos;, uppercase preferred, spelled out (no abbreviation), in place of a street address</skos:definition>
		<fibo-fnd-utl-av:explanatoryNote>The value of the +4 component of a ZIP+4 code should be &apos;9999&apos;.</fibo-fnd-utl-av:explanatoryNote>
	</owl:Class>
	
	<owl:Class rdf:about="&fibo-fbc-fct-uspsaa;GeographicDirectionalSymbol">
		<rdfs:subClassOf rdf:resource="&fibo-fnd-arr-cd;CodeElement"/>
		<rdfs:subClassOf>
			<owl:Restriction>
				<owl:onProperty rdf:resource="&fibo-fnd-rel-rel;hasTag"/>
				<owl:someValuesFrom rdf:resource="&xsd;string"/>
			</owl:Restriction>
		</rdfs:subClassOf>
		<rdfs:label>geographic directional symbol</rdfs:label>
		<owl:equivalentClass>
			<owl:Class>
				<owl:oneOf rdf:parseType="Collection">
					<rdf:Description rdf:about="&fibo-fbc-fct-uspsaa;East">
					</rdf:Description>
					<rdf:Description rdf:about="&fibo-fbc-fct-uspsaa;North">
					</rdf:Description>
					<rdf:Description rdf:about="&fibo-fbc-fct-uspsaa;Northeast">
					</rdf:Description>
					<rdf:Description rdf:about="&fibo-fbc-fct-uspsaa;Northwest">
					</rdf:Description>
					<rdf:Description rdf:about="&fibo-fbc-fct-uspsaa;South">
					</rdf:Description>
					<rdf:Description rdf:about="&fibo-fbc-fct-uspsaa;Southeast">
					</rdf:Description>
					<rdf:Description rdf:about="&fibo-fbc-fct-uspsaa;Southwest">
					</rdf:Description>
					<rdf:Description rdf:about="&fibo-fbc-fct-uspsaa;West">
					</rdf:Description>
				</owl:oneOf>
			</owl:Class>
		</owl:equivalentClass>
		<skos:definition>code element that gives directional information for delivery (i.e., N, S, E, W, NE, NW, SE, SW)</skos:definition>
	</owl:Class>
	
	<owl:Class rdf:about="&fibo-fbc-fct-uspsaa;HighwayContractRoute">
		<rdfs:subClassOf rdf:resource="&fibo-fbc-fct-uspsaa;SupplementalAddress"/>
		<rdfs:subClassOf>
			<owl:Restriction>
				<owl:onProperty rdf:resource="&fibo-fnd-arr-arr;hasConstituent"/>
				<owl:hasValue rdf:resource="&fibo-fbc-fct-uspsaa;HighwayContractRouteDesignator"/>
			</owl:Restriction>
		</rdfs:subClassOf>
		<rdfs:label>highway contract route</rdfs:label>
		<skos:definition>highway contract route associated with an address</skos:definition>
	</owl:Class>
	
	<owl:Class rdf:about="&fibo-fbc-fct-uspsaa;HighwayContractRouteAddress">
		<rdfs:subClassOf rdf:resource="&fibo-fbc-fct-uspsaa;DeliveryAddress"/>
		<rdfs:subClassOf>
			<owl:Restriction>
				<owl:onProperty rdf:resource="&fibo-fnd-arr-arr;hasConstituent"/>
				<owl:onClass rdf:resource="&fibo-fbc-fct-uspsaa;HighwayContractRoute"/>
				<owl:qualifiedCardinality rdf:datatype="&xsd;nonNegativeInteger">1</owl:qualifiedCardinality>
			</owl:Restriction>
		</rdfs:subClassOf>
		<rdfs:subClassOf>
			<owl:Restriction>
				<owl:onProperty rdf:resource="&fibo-fnd-arr-arr;hasConstituent"/>
				<owl:onClass rdf:resource="&fibo-fbc-fct-uspsaa;Mailbox"/>
				<owl:qualifiedCardinality rdf:datatype="&xsd;nonNegativeInteger">1</owl:qualifiedCardinality>
			</owl:Restriction>
		</rdfs:subClassOf>
		<rdfs:label>highway contract address</rdfs:label>
		<owl:disjointWith rdf:resource="&fibo-fbc-fct-uspsaa;ConventionalDeliveryAddress"/>
		<skos:definition>delivery address whose delivery address line uses the abbreviation &apos;HC&apos;, followed by the route identifier, followed by &apos;BOX&apos; followed by box number, in place of a street address</skos:definition>
	</owl:Class>
	
	<owl:NamedIndividual rdf:about="&fibo-fbc-fct-uspsaa;HighwayContractRouteDesignator">
		<rdf:type rdf:resource="&fibo-fbc-fct-uspsaa;SupplementalAddressDesignator"/>
		<rdfs:label>highway contract route designator</rdfs:label>
		<skos:definition>designator for a route served by an independent contractor rather than directly by the U.S. Postal Service</skos:definition>
		<fibo-fbc-fct-uspsaa:preferredAbbreviation>HC</fibo-fbc-fct-uspsaa:preferredAbbreviation>
	</owl:NamedIndividual>
	
	<owl:Class rdf:about="&fibo-fbc-fct-uspsaa;InternationalAddress">
		<rdfs:subClassOf rdf:resource="&fibo-fbc-fct-uspsaa;ConventionalDeliveryAddress"/>
		<rdfs:subClassOf>
			<owl:Restriction>
				<owl:onProperty rdf:resource="&fibo-fbc-fct-breg;hasCountry"/>
				<owl:onClass rdf:resource="&lcc-cr;Country"/>
				<owl:qualifiedCardinality rdf:datatype="&xsd;nonNegativeInteger">1</owl:qualifiedCardinality>
			</owl:Restriction>
		</rdfs:subClassOf>
		<rdfs:label>international address</rdfs:label>
		<skos:definition>delivery address intended for delivery outside the United States or Canada</skos:definition>
	</owl:Class>
	
	<owl:Class rdf:about="&fibo-fbc-fct-uspsaa;Mailbox">
		<rdfs:subClassOf rdf:resource="&fibo-fbc-fct-uspsaa;SupplementalAddress"/>
		<rdfs:subClassOf>
			<owl:Restriction>
				<owl:onProperty rdf:resource="&fibo-fnd-arr-arr;hasConstituent"/>
				<owl:hasValue rdf:resource="&fibo-fbc-fct-uspsaa;MailboxDesignator"/>
			</owl:Restriction>
		</rdfs:subClassOf>
		<rdfs:label>mailbox</rdfs:label>
		<skos:definition>mailbox, other than a U.S. Post Office box, associated with an address</skos:definition>
	</owl:Class>
	
	<owl:NamedIndividual rdf:about="&fibo-fbc-fct-uspsaa;MailboxDesignator">
		<rdf:type rdf:resource="&fibo-fbc-fct-uspsaa;SupplementalAddressDesignator"/>
		<rdfs:label>mailbox designator</rdfs:label>
		<skos:definition>designator for a mail box other than a U.S. Post Office box</skos:definition>
		<fibo-fbc-fct-uspsaa:preferredAbbreviation>BOX</fibo-fbc-fct-uspsaa:preferredAbbreviation>
	</owl:NamedIndividual>
	
	<owl:NamedIndividual rdf:about="&fibo-fbc-fct-uspsaa;North">
		<rdf:type rdf:resource="&fibo-fbc-fct-uspsaa;GeographicDirectionalSymbol"/>
		<rdfs:label xml:lang="es">Norte</rdfs:label>
		<rdfs:label xml:lang="en">North</rdfs:label>
		<skos:definition>geographic directional symbol for North</skos:definition>
		<fibo-fnd-rel-rel:hasTag>N</fibo-fnd-rel-rel:hasTag>
	</owl:NamedIndividual>
	
	<owl:NamedIndividual rdf:about="&fibo-fbc-fct-uspsaa;Northeast">
		<rdf:type rdf:resource="&fibo-fbc-fct-uspsaa;GeographicDirectionalSymbol"/>
		<rdfs:label xml:lang="es">Noreste</rdfs:label>
		<rdfs:label xml:lang="en">Northeast</rdfs:label>
		<skos:definition>geographic directional symbol for Northeast</skos:definition>
		<fibo-fnd-rel-rel:hasTag>NE</fibo-fnd-rel-rel:hasTag>
	</owl:NamedIndividual>
	
	<owl:NamedIndividual rdf:about="&fibo-fbc-fct-uspsaa;Northwest">
		<rdf:type rdf:resource="&fibo-fbc-fct-uspsaa;GeographicDirectionalSymbol"/>
		<rdfs:label xml:lang="es">Noroeste</rdfs:label>
		<rdfs:label xml:lang="en">Northwest</rdfs:label>
		<skos:definition>geographic directional symbol for Northwest</skos:definition>
		<fibo-fnd-rel-rel:hasTag>NO</fibo-fnd-rel-rel:hasTag>
		<fibo-fnd-rel-rel:hasTag>NW</fibo-fnd-rel-rel:hasTag>
	</owl:NamedIndividual>
	
	<owl:Class rdf:about="&fibo-fbc-fct-uspsaa;OverseasMilitaryAddress">
		<rdfs:subClassOf rdf:resource="&fibo-fbc-fct-uspsaa;DeliveryAddress"/>
		<rdfs:label>overseas military address</rdfs:label>
		<owl:disjointWith rdf:resource="&fibo-fbc-fct-uspsaa;ConventionalDeliveryAddress"/>
		<skos:definition>delivery address whose delivery address line uses an abbreviation for the unit or command such as &apos;CMR&apos;, &apos;PSC&apos;, or &apos;UNIT&apos;, or  &apos;HC&apos;, followed by the unit identifier, followed by &apos;BOX&apos; followed by box number, in place of a street address, either &apos;APO&apos; or &apos;FPO&apos; as the literal value for the city and the appropriate armed forces subdivision code in place of a subdivision (state) code</skos:definition>
	</owl:Class>
	
	<owl:Class rdf:about="&fibo-fbc-fct-uspsaa;PostOfficeBox">
		<rdfs:subClassOf rdf:resource="&fibo-fbc-fct-uspsaa;SupplementalAddress"/>
		<rdfs:subClassOf>
			<owl:Restriction>
				<owl:onProperty rdf:resource="&fibo-fnd-arr-arr;hasConstituent"/>
				<owl:hasValue rdf:resource="&fibo-fbc-fct-uspsaa;PostOfficeBoxDesignator"/>
			</owl:Restriction>
		</rdfs:subClassOf>
		<rdfs:label>post office box</rdfs:label>
		<skos:definition>U.S. post office box associated with an address</skos:definition>
	</owl:Class>
	
	<owl:Class rdf:about="&fibo-fbc-fct-uspsaa;PostOfficeBoxAddress">
		<rdfs:subClassOf rdf:resource="&fibo-fbc-fct-uspsaa;DeliveryAddress"/>
		<rdfs:subClassOf>
			<owl:Restriction>
				<owl:onProperty rdf:resource="&fibo-fnd-arr-arr;hasConstituent"/>
				<owl:onClass rdf:resource="&fibo-fbc-fct-uspsaa;PostOfficeBox"/>
				<owl:qualifiedCardinality rdf:datatype="&xsd;nonNegativeInteger">1</owl:qualifiedCardinality>
			</owl:Restriction>
		</rdfs:subClassOf>
		<rdfs:label>post office box address</rdfs:label>
		<owl:disjointWith rdf:resource="&fibo-fbc-fct-uspsaa;ConventionalDeliveryAddress"/>
		<skos:definition>delivery address whose delivery address line uses the abbreviation &apos;PO&apos;, followed by &apos;BOX&apos; followed by the box number, in place of a street address</skos:definition>
	</owl:Class>
	
	<owl:NamedIndividual rdf:about="&fibo-fbc-fct-uspsaa;PostOfficeBoxDesignator">
		<rdf:type rdf:resource="&fibo-fbc-fct-uspsaa;SupplementalAddressDesignator"/>
		<rdfs:label>post office box designator</rdfs:label>
		<skos:definition>designator for a U.S. Post Office box</skos:definition>
		<fibo-fbc-fct-uspsaa:preferredAbbreviation>PO BOX</fibo-fbc-fct-uspsaa:preferredAbbreviation>
	</owl:NamedIndividual>
	
	<owl:Class rdf:about="&fibo-fbc-fct-uspsaa;Postcode">
		<rdfs:subClassOf rdf:resource="&fibo-fnd-arr-cd;CodeElement"/>
		<rdfs:subClassOf rdf:resource="&fibo-fnd-arr-id;Identifier"/>
		<rdfs:subClassOf>
			<owl:Restriction>
				<owl:onProperty rdf:resource="&fibo-fnd-rel-rel;hasTag"/>
				<owl:onDataRange rdf:resource="&xsd;string"/>
				<owl:qualifiedCardinality rdf:datatype="&xsd;nonNegativeInteger">1</owl:qualifiedCardinality>
			</owl:Restriction>
		</rdfs:subClassOf>
		<rdfs:label>postcode</rdfs:label>
		<skos:definition>group of numbers or letters and numbers which are added to a postal address to assist the sorting of mail</skos:definition>
		<fibo-fnd-utl-av:synonym>postal code</fibo-fnd-utl-av:synonym>
	</owl:Class>
	
	<owl:Class rdf:about="&fibo-fbc-fct-uspsaa;PostdirectionalSymbol">
		<rdfs:subClassOf rdf:resource="&fibo-fbc-fct-uspsaa;GeographicDirectionalSymbol"/>
		<rdfs:label>postdirectional symbol</rdfs:label>
		<skos:definition>geographic directional symbol that follows the street name and street suffix in a street address</skos:definition>
		<fibo-fnd-utl-av:explanatoryNote>Note that when two directionals appear consecutively as one or two words following the street name or suffix, then they become the postdirectional (together). If the directional word appears between the street name and the suffix, then it should be considered part of the primary street name.</fibo-fnd-utl-av:explanatoryNote>
	</owl:Class>
	
	<owl:Class rdf:about="&fibo-fbc-fct-uspsaa;PredirectionalSymbol">
		<rdfs:subClassOf rdf:resource="&fibo-fbc-fct-uspsaa;GeographicDirectionalSymbol"/>
		<rdfs:label>predirectional symbol</rdfs:label>
		<skos:definition>geographic directional symbol that occurs after the primary street number but before the street name in a street address</skos:definition>
		<fibo-fnd-utl-av:explanatoryNote>Note that when two directionals appear consecutively as one or two words before the street name, then they become the predirectional (together). Exceptions are any combinations of NORTH-SOUTH or EAST-WEST as consecutive words. In these cases the second directional becomes part of the primary street name.</fibo-fnd-utl-av:explanatoryNote>
	</owl:Class>
	
	<owl:Class rdf:about="&fibo-fbc-fct-uspsaa;PrimaryAddressNumber">
		<rdfs:subClassOf rdf:resource="&fibo-fbc-fct-uspsaa;AddressComponent"/>
		<rdfs:subClassOf>
			<owl:Restriction>
				<owl:onProperty rdf:resource="&fibo-fnd-rel-rel;hasTag"/>
				<owl:onDataRange rdf:resource="&xsd;string"/>
				<owl:qualifiedCardinality rdf:datatype="&xsd;nonNegativeInteger">1</owl:qualifiedCardinality>
			</owl:Restriction>
		</rdfs:subClassOf>
		<rdfs:label>primary address number</rdfs:label>
		<skos:definition>index to a location that identifies a building with respect to a given street</skos:definition>
	</owl:Class>
	
	<owl:Class rdf:about="&fibo-fbc-fct-uspsaa;PrivateMailBoxAddress">
		<rdfs:subClassOf rdf:resource="&fibo-fbc-fct-uspsaa;ConventionalDeliveryAddress"/>
		<rdfs:label>private mail box address</rdfs:label>
		<skos:definition>delivery address provided by a commercial mail receiving company that includes a supplementary address line containing the abbreviation &apos;PMB&apos; or the pound &quot;#&quot; symbol followed by the mailbox number; alternatively, &apos;PMB&apos; or &apos;#&quot; and the mailbox number can be appended to the street address</skos:definition>
	</owl:Class>
	
	<owl:Class rdf:about="&fibo-fbc-fct-uspsaa;PuertoRicoAddress">
		<rdfs:subClassOf rdf:resource="&fibo-fbc-fct-uspsaa;DeliveryAddress"/>
		<rdfs:subClassOf>
			<owl:Restriction>
				<owl:onProperty rdf:resource="&fibo-fnd-arr-arr;hasConstituent"/>
				<owl:onClass rdf:resource="&fibo-fbc-fct-uspsaa;StreetAddress"/>
				<owl:maxQualifiedCardinality rdf:datatype="&xsd;nonNegativeInteger">1</owl:maxQualifiedCardinality>
			</owl:Restriction>
		</rdfs:subClassOf>
		<rdfs:subClassOf>
			<owl:Restriction>
				<owl:onProperty rdf:resource="&fibo-fnd-arr-arr;hasConstituent"/>
				<owl:onClass rdf:resource="&fibo-fbc-fct-uspsaa;Urbanization"/>
				<owl:maxQualifiedCardinality rdf:datatype="&xsd;nonNegativeInteger">1</owl:maxQualifiedCardinality>
			</owl:Restriction>
		</rdfs:subClassOf>
		<rdfs:label>Puerto Rico address</rdfs:label>
		<skos:definition>delivery address for a delivery point in Puerto Rico that may include a supplementary address line containing the abbreviation &apos;URB&apos; followed by the name of the urbanization area that is appropriate for that address</skos:definition>
	</owl:Class>
	
	<owl:Class rdf:about="&fibo-fbc-fct-uspsaa;RuralRoute">
		<rdfs:subClassOf rdf:resource="&fibo-fbc-fct-uspsaa;SupplementalAddress"/>
		<rdfs:subClassOf>
			<owl:Restriction>
				<owl:onProperty rdf:resource="&fibo-fnd-arr-arr;hasConstituent"/>
				<owl:hasValue rdf:resource="&fibo-fbc-fct-uspsaa;RuralRouteDesignator"/>
			</owl:Restriction>
		</rdfs:subClassOf>
		<rdfs:label>highway contract route address</rdfs:label>
		<skos:definition>mail route outside the city or township limits in a rural area associated with an address</skos:definition>
	</owl:Class>
	
	<owl:Class rdf:about="&fibo-fbc-fct-uspsaa;RuralRouteAddress">
		<rdfs:subClassOf rdf:resource="&fibo-fbc-fct-uspsaa;DeliveryAddress"/>
		<rdfs:subClassOf>
			<owl:Restriction>
				<owl:onProperty rdf:resource="&fibo-fnd-arr-arr;hasConstituent"/>
				<owl:onClass rdf:resource="&fibo-fbc-fct-uspsaa;Mailbox"/>
				<owl:qualifiedCardinality rdf:datatype="&xsd;nonNegativeInteger">1</owl:qualifiedCardinality>
			</owl:Restriction>
		</rdfs:subClassOf>
		<rdfs:subClassOf>
			<owl:Restriction>
				<owl:onProperty rdf:resource="&fibo-fnd-arr-arr;hasConstituent"/>
				<owl:onClass rdf:resource="&fibo-fbc-fct-uspsaa;RuralRoute"/>
				<owl:qualifiedCardinality rdf:datatype="&xsd;nonNegativeInteger">1</owl:qualifiedCardinality>
			</owl:Restriction>
		</rdfs:subClassOf>
		<rdfs:label>rural route address</rdfs:label>
		<owl:disjointWith rdf:resource="&fibo-fbc-fct-uspsaa;ConventionalDeliveryAddress"/>
		<skos:definition>delivery address whose delivery address line uses the abbreviation &apos;RR&apos;, followed by the route identifier, followed by &apos;BOX&apos; followed by box number, in place of a street address</skos:definition>
	</owl:Class>
	
	<owl:NamedIndividual rdf:about="&fibo-fbc-fct-uspsaa;RuralRouteDesignator">
		<rdf:type rdf:resource="&fibo-fbc-fct-uspsaa;SupplementalAddressDesignator"/>
		<rdfs:label>rural route designator</rdfs:label>
		<skos:definition>designator for a mail route outside the city or township limits in a rural area</skos:definition>
		<fibo-fbc-fct-uspsaa:preferredAbbreviation>RR</fibo-fbc-fct-uspsaa:preferredAbbreviation>
	</owl:NamedIndividual>
	
	<owl:Class rdf:about="&fibo-fbc-fct-uspsaa;SecondaryUnit">
		<rdfs:subClassOf rdf:resource="&fibo-fbc-fct-uspsaa;AddressComponent"/>
		<rdfs:subClassOf>
			<owl:Restriction>
				<owl:onProperty rdf:resource="&fibo-fnd-arr-arr;hasConstituent"/>
				<owl:onClass rdf:resource="&fibo-fbc-fct-uspsaa;SecondaryUnitIndicator"/>
				<owl:maxQualifiedCardinality rdf:datatype="&xsd;nonNegativeInteger">1</owl:maxQualifiedCardinality>
			</owl:Restriction>
		</rdfs:subClassOf>
		<rdfs:subClassOf>
			<owl:Restriction>
				<owl:onProperty rdf:resource="&fibo-fnd-arr-arr;hasConstituent"/>
				<owl:onClass rdf:resource="&fibo-fbc-fct-uspsaa;SecondaryUnitDesignator"/>
				<owl:qualifiedCardinality rdf:datatype="&xsd;nonNegativeInteger">1</owl:qualifiedCardinality>
			</owl:Restriction>
		</rdfs:subClassOf>
		<rdfs:label>secondary unit</rdfs:label>
		<skos:definition>index to a location that identifies an individual secondary unit at a given street address</skos:definition>
	</owl:Class>
	
	<owl:Class rdf:about="&fibo-fbc-fct-uspsaa;SecondaryUnitDesignator">
		<rdfs:subClassOf rdf:resource="&fibo-fnd-arr-cls;Classifier"/>
		<rdfs:subClassOf>
			<owl:Restriction>
				<owl:onProperty rdf:resource="&fibo-fbc-fct-uspsaa;requiresSecondaryUnitRange"/>
				<owl:onDataRange rdf:resource="&xsd;boolean"/>
				<owl:qualifiedCardinality rdf:datatype="&xsd;nonNegativeInteger">1</owl:qualifiedCardinality>
			</owl:Restriction>
		</rdfs:subClassOf>
		<rdfs:label>secondary unit designator</rdfs:label>
		<skos:definition>classifier for a smaller structure or component within a larger facility, such as an apartment, office, mail stop, or other similar designation</skos:definition>
		<fibo-fnd-utl-av:explanatoryNote>Note that only certain secondary units require a secondary range, such as an apartment number, to complete a delivery point.</fibo-fnd-utl-av:explanatoryNote>
	</owl:Class>
	
	<owl:Class rdf:about="&fibo-fbc-fct-uspsaa;SecondaryUnitIndicator">
		<rdfs:subClassOf rdf:resource="&fibo-fbc-fct-uspsaa;AddressComponent"/>
		<rdfs:subClassOf>
			<owl:Restriction>
				<owl:onProperty rdf:resource="&fibo-fnd-rel-rel;hasTag"/>
				<owl:onDataRange rdf:resource="&xsd;string"/>
				<owl:qualifiedCardinality rdf:datatype="&xsd;nonNegativeInteger">1</owl:qualifiedCardinality>
			</owl:Restriction>
		</rdfs:subClassOf>
		<rdfs:label>secondary unit indicator</rdfs:label>
		<skos:definition>index to the specific unit within a secondary unit, such as a building or apartment, at a particular street address</skos:definition>
	</owl:Class>
	
	<owl:NamedIndividual rdf:about="&fibo-fbc-fct-uspsaa;South">
		<rdf:type rdf:resource="&fibo-fbc-fct-uspsaa;GeographicDirectionalSymbol"/>
		<rdfs:label xml:lang="en">South</rdfs:label>
		<rdfs:label xml:lang="es">Sur</rdfs:label>
		<skos:definition>geographic directional symbol for South</skos:definition>
		<fibo-fnd-rel-rel:hasTag>S</fibo-fnd-rel-rel:hasTag>
	</owl:NamedIndividual>
	
	<owl:NamedIndividual rdf:about="&fibo-fbc-fct-uspsaa;Southeast">
		<rdf:type rdf:resource="&fibo-fbc-fct-uspsaa;GeographicDirectionalSymbol"/>
		<rdfs:label xml:lang="en">Southeast</rdfs:label>
		<rdfs:label xml:lang="es">Sureste</rdfs:label>
		<skos:definition>geographic directional symbol for Southeast</skos:definition>
		<fibo-fnd-rel-rel:hasTag>SE</fibo-fnd-rel-rel:hasTag>
	</owl:NamedIndividual>
	
	<owl:NamedIndividual rdf:about="&fibo-fbc-fct-uspsaa;Southwest">
		<rdf:type rdf:resource="&fibo-fbc-fct-uspsaa;GeographicDirectionalSymbol"/>
		<rdfs:label xml:lang="en">Southwest</rdfs:label>
		<rdfs:label xml:lang="es">Suroeste</rdfs:label>
		<skos:definition>geographic directional symbol for Southwest</skos:definition>
		<fibo-fnd-rel-rel:hasTag>SO</fibo-fnd-rel-rel:hasTag>
		<fibo-fnd-rel-rel:hasTag>SW</fibo-fnd-rel-rel:hasTag>
	</owl:NamedIndividual>
	
	<owl:Class rdf:about="&fibo-fbc-fct-uspsaa;StandardizedAddress">
		<rdfs:subClassOf rdf:resource="&fibo-fbc-fct-uspsaa;DeliveryAddress"/>
		<rdfs:label>standardized address</rdfs:label>
		<skos:definition>delivery address that is fully spelled out, abbreviated by using the Postal Service standard abbreviations or as given in the current Postal Service ZIP+4 file</skos:definition>
	</owl:Class>
	
	<owl:Class rdf:about="&fibo-fbc-fct-uspsaa;StreetAddress">
		<rdfs:subClassOf rdf:resource="&fibo-fbc-fct-uspsaa;AddressComponent"/>
		<rdfs:subClassOf>
			<owl:Restriction>
				<owl:onProperty rdf:resource="&fibo-fnd-arr-arr;hasConstituent"/>
				<owl:onClass rdf:resource="&fibo-fbc-fct-uspsaa;SecondaryUnit"/>
				<owl:maxQualifiedCardinality rdf:datatype="&xsd;nonNegativeInteger">1</owl:maxQualifiedCardinality>
			</owl:Restriction>
		</rdfs:subClassOf>
		<rdfs:subClassOf>
			<owl:Restriction>
				<owl:onProperty rdf:resource="&fibo-fnd-arr-arr;hasConstituent"/>
				<owl:onClass rdf:resource="&fibo-fbc-fct-uspsaa;StreetSuffix"/>
				<owl:maxQualifiedCardinality rdf:datatype="&xsd;nonNegativeInteger">1</owl:maxQualifiedCardinality>
			</owl:Restriction>
		</rdfs:subClassOf>
		<rdfs:subClassOf>
			<owl:Restriction>
				<owl:onProperty rdf:resource="&fibo-fnd-arr-arr;hasConstituent"/>
				<owl:onClass rdf:resource="&fibo-fbc-fct-uspsaa;PostdirectionalSymbol"/>
				<owl:maxQualifiedCardinality rdf:datatype="&xsd;nonNegativeInteger">2</owl:maxQualifiedCardinality>
			</owl:Restriction>
		</rdfs:subClassOf>
		<rdfs:subClassOf>
			<owl:Restriction>
				<owl:onProperty rdf:resource="&fibo-fnd-arr-arr;hasConstituent"/>
				<owl:onClass rdf:resource="&fibo-fbc-fct-uspsaa;PredirectionalSymbol"/>
				<owl:maxQualifiedCardinality rdf:datatype="&xsd;nonNegativeInteger">2</owl:maxQualifiedCardinality>
			</owl:Restriction>
		</rdfs:subClassOf>
		<rdfs:subClassOf>
			<owl:Restriction>
				<owl:onProperty rdf:resource="&fibo-fnd-arr-arr;hasConstituent"/>
				<owl:onClass rdf:resource="&fibo-fbc-fct-uspsaa;PrimaryAddressNumber"/>
				<owl:qualifiedCardinality rdf:datatype="&xsd;nonNegativeInteger">1</owl:qualifiedCardinality>
			</owl:Restriction>
		</rdfs:subClassOf>
		<rdfs:subClassOf>
			<owl:Restriction>
				<owl:onProperty rdf:resource="&fibo-fnd-arr-arr;hasConstituent"/>
				<owl:onClass rdf:resource="&fibo-fbc-fct-uspsaa;StreetName"/>
				<owl:qualifiedCardinality rdf:datatype="&xsd;nonNegativeInteger">1</owl:qualifiedCardinality>
			</owl:Restriction>
		</rdfs:subClassOf>
		<rdfs:label>street address</rdfs:label>
		<skos:definition>index to a location that consists of a primary address number, predirectional, street name, suffix, postdirectional, and an optional secondary unit</skos:definition>
		<fibo-fnd-utl-av:explanatoryNote>If the street address represents a single mailbox, residence, office, or other secondary unit, then it qualifies as a unique delivery address.</fibo-fnd-utl-av:explanatoryNote>
	</owl:Class>
	
	<owl:Class rdf:about="&fibo-fbc-fct-uspsaa;StreetName">
		<rdfs:subClassOf rdf:resource="&fibo-fbc-fct-uspsaa;AddressComponent"/>
		<rdfs:subClassOf rdf:resource="&fibo-fnd-arr-id;Identifier"/>
		<rdfs:label>street name</rdfs:label>
		<skos:definition>identifier for a street in some context (e.g., city, municipality, geographic region)</skos:definition>
	</owl:Class>
	
	<owl:Class rdf:about="&fibo-fbc-fct-uspsaa;StreetSuffix">
		<rdfs:subClassOf rdf:resource="&fibo-fbc-fct-uspsaa;AddressComponent"/>
		<rdfs:subClassOf rdf:resource="&fibo-fnd-arr-cls;Classifier"/>
		<rdfs:label>street suffix</rdfs:label>
		<skos:definition>classifier for a street or other delivery location, such as a dwelling located along a waterway</skos:definition>
		<fibo-fnd-utl-av:explanatoryNote>The suffix may provide some insight into the size or length of the street, though not necessarily consistently. In some cities, the suffix differentiates the street from another in the same context, such as 19th Street vs. 19th Avenue in San Francisco.</fibo-fnd-utl-av:explanatoryNote>
	</owl:Class>
	
	<owl:Class rdf:about="&fibo-fbc-fct-uspsaa;SupplementalAddress">
		<rdfs:subClassOf rdf:resource="&fibo-fbc-fct-uspsaa;AddressComponent"/>
		<rdfs:subClassOf>
			<owl:Restriction>
				<owl:onProperty rdf:resource="&fibo-fnd-arr-arr;hasConstituent"/>
				<owl:onClass rdf:resource="&fibo-fbc-fct-uspsaa;SupplementalAddressIndicatorOrUnit"/>
				<owl:maxQualifiedCardinality rdf:datatype="&xsd;nonNegativeInteger">1</owl:maxQualifiedCardinality>
			</owl:Restriction>
		</rdfs:subClassOf>
		<rdfs:subClassOf>
			<owl:Restriction>
				<owl:onProperty rdf:resource="&fibo-fnd-arr-arr;hasConstituent"/>
				<owl:onClass rdf:resource="&fibo-fbc-fct-uspsaa;SupplementalAddressDesignator"/>
				<owl:qualifiedCardinality rdf:datatype="&xsd;nonNegativeInteger">1</owl:qualifiedCardinality>
			</owl:Restriction>
		</rdfs:subClassOf>
		<rdfs:label>supplemental address</rdfs:label>
		<skos:definition>index to a location that provides supplementary information relevant to an address</skos:definition>
	</owl:Class>
	
	<owl:Class rdf:about="&fibo-fbc-fct-uspsaa;SupplementalAddressDesignator">
		<rdfs:subClassOf rdf:resource="&fibo-fnd-arr-cls;Classifier"/>
		<rdfs:label>supplemental address designator</rdfs:label>
		<skos:definition>classifier for supplemental information, such as a highway contract route, rural route, condominium complex, mail box, or other similar designation</skos:definition>
	</owl:Class>
	
	<owl:Class rdf:about="&fibo-fbc-fct-uspsaa;SupplementalAddressIndicatorOrUnit">
		<rdfs:subClassOf rdf:resource="&fibo-fbc-fct-uspsaa;AddressComponent"/>
		<rdfs:subClassOf>
			<owl:Restriction>
				<owl:onProperty rdf:resource="&fibo-fnd-rel-rel;hasTag"/>
				<owl:onDataRange rdf:resource="&xsd;string"/>
				<owl:qualifiedCardinality rdf:datatype="&xsd;nonNegativeInteger">1</owl:qualifiedCardinality>
			</owl:Restriction>
		</rdfs:subClassOf>
		<rdfs:label>secondary unit indicator</rdfs:label>
		<skos:definition>index to the specific route, box, condominium or other indicator or unit associated with a specific address</skos:definition>
	</owl:Class>
	
	<owl:NamedIndividual rdf:about="&fibo-fbc-fct-uspsaa;UnitedStatesPostalService">
		<rdf:type rdf:resource="&fibo-be-ge-ge;GovernmentAgency"/>
		<rdfs:label>United States Postal Service</rdfs:label>
		<skos:definition>United States Postal Service (USPS), a self-supporting, independent federal agency whose mission is to provide a reliable, efficient, trusted and affordable universal delivery service that connects people and helps businesses grow</skos:definition>
		<fibo-be-ge-ge:hasJurisdiction rdf:resource="&fibo-be-ge-usj;UnitedStatesJurisdiction"/>
		<fibo-fbc-fct-breg:hasWebsite rdf:datatype="&xsd;anyURI">https://www.usps.com/</fibo-fbc-fct-breg:hasWebsite>
		<fibo-fnd-plc-cty:hasCoverageArea rdf:resource="&lcc-3166-1;UnitedStatesOfAmerica"/>
		<fibo-fnd-rel-rel:isPartOf rdf:resource="&fibo-be-ge-ge;ExecutiveBranch"/>
		<fibo-fnd-rel-rel:isPartOf rdf:resource="&fibo-be-ge-usj;UnitedStatesGovernment"/>
		<fibo-fnd-utl-av:abbreviation>U.S. Postal Service</fibo-fnd-utl-av:abbreviation>
		<fibo-fnd-utl-av:abbreviation>USPS</fibo-fnd-utl-av:abbreviation>
		<fibo-fnd-utl-av:explanatoryNote>With more than 31,600 retail locations and the most frequently visited website in the federal government, usps.com, the Postal Service has annual revenue of nearly $69 billion and delivers 47 percent of the world&apos;s mail.</fibo-fnd-utl-av:explanatoryNote>
	</owl:NamedIndividual>
	
	<owl:NamedIndividual rdf:about="&fibo-fbc-fct-uspsaa;UnitedStatesPostalServicesRegulator">
		<rdf:type rdf:resource="&fibo-fbc-fct-ra;RegistrationAuthority"/>
		<rdf:type rdf:resource="&fibo-fbc-fct-rga;RegulatoryAgency"/>
		<rdfs:label>United States postal services regulator</rdfs:label>
		<skos:definition>regulatory agency and registration authority role of the U.S. Postal Service</skos:definition>
		<fibo-fnd-rel-rel:hasIdentity rdf:resource="&fibo-fbc-fct-uspsaa;UnitedStatesPostalService"/>
	</owl:NamedIndividual>
	
	<owl:Class rdf:about="&fibo-fbc-fct-uspsaa;Urbanization">
		<rdfs:subClassOf rdf:resource="&lcc-cr;CountrySubdivision"/>
		<rdfs:label>urbanization</rdfs:label>
		<skos:definition>an area, sector, or development within a geographic area</skos:definition>
		<fibo-fnd-utl-av:explanatoryNote>This URB descriptor, commonly used in urban areas of Puerto Rico, is an important part of the addressing format, as it describes the location of a given street.</fibo-fnd-utl-av:explanatoryNote>
	</owl:Class>
	
	<owl:NamedIndividual rdf:about="&fibo-fbc-fct-uspsaa;West">
		<rdf:type rdf:resource="&fibo-fbc-fct-uspsaa;GeographicDirectionalSymbol"/>
		<rdfs:label xml:lang="es">Oeste</rdfs:label>
		<rdfs:label xml:lang="en">West</rdfs:label>
		<skos:definition>geographic directional symbol for West</skos:definition>
		<fibo-fnd-rel-rel:hasTag>O</fibo-fnd-rel-rel:hasTag>
		<fibo-fnd-rel-rel:hasTag>W</fibo-fnd-rel-rel:hasTag>
	</owl:NamedIndividual>
	
	<owl:Class rdf:about="&fibo-fbc-fct-uspsaa;ZIPCode">
		<rdfs:subClassOf rdf:resource="&fibo-fbc-fct-uspsaa;Postcode"/>
		<rdfs:label>Zip Code</rdfs:label>
		<skos:definition>five-digit code code assigned to a delivery address indicating the state and post office or postal zone</skos:definition>
	</owl:Class>
	
	<owl:Class rdf:about="&fibo-fbc-fct-uspsaa;ZIPPlus4Code">
		<rdfs:subClassOf rdf:resource="&fibo-fbc-fct-uspsaa;Postcode"/>
		<rdfs:label>ZIP+4 Code</rdfs:label>
		<skos:definition>nine-digit number consisting of five digits, a hyphen, and four digits, which the USPS describes by its trademark ZIP+4</skos:definition>
		<fibo-fnd-utl-av:explanatoryNote>The correct format for a numeric ZIP+4 code is five digits, a hyphen, and four digits. The first five digits represent the 5-digit ZIP Code; the sixth and seventh digits (the first two after the hyphen) identify an area known as a sector; the eighth and ninth digits identify a smaller area known as a segment. Together, the final four digits identify geographic units such as a side of a street between intersections, both sides of a street between intersections, a building, a floor or group of floors in a building, a firm within a building, a span of boxes on a rural route, or a group of Post Office boxes to which a single USPS employee makes delivery.</fibo-fnd-utl-av:explanatoryNote>
	</owl:Class>
	
	<owl:Class rdf:about="&fibo-fbc-fct-uspsaa;ZipCodeScheme">
		<rdfs:subClassOf rdf:resource="&fibo-fnd-arr-cd;CodeSet"/>
		<rdfs:subClassOf rdf:resource="&fibo-fnd-arr-id;IdentificationScheme"/>
		<rdfs:subClassOf>
			<owl:Restriction>
				<owl:onProperty rdf:resource="&fibo-fnd-rel-rel;hasMember"/>
				<owl:someValuesFrom>
					<owl:Class>
						<owl:unionOf rdf:parseType="Collection">
							<rdf:Description rdf:about="&fibo-fbc-fct-uspsaa;ZIPCode">
							</rdf:Description>
							<rdf:Description rdf:about="&fibo-fbc-fct-uspsaa;ZIPPlus4Code">
							</rdf:Description>
						</owl:unionOf>
					</owl:Class>
				</owl:someValuesFrom>
			</owl:Restriction>
		</rdfs:subClassOf>
		<rdfs:label>zip code scheme</rdfs:label>
		<rdfs:seeAlso rdf:resource="https://pe.usps.com/cpim/ftp/pubs/Pub28/pub28.pdf"/>
		<skos:definition>system used in the U.S. to facilitate the delivery of mail, consisting of a five- or nine-digit code printed directly after the address, the first five digits (initial code) indicating the state and post office or postal zone, the last four (expanded code) the box section or number, portion of a rural route, building, or other specific delivery location</skos:definition>
	</owl:Class>
	
	<owl:AnnotationProperty rdf:about="&fibo-fbc-fct-uspsaa;commonAbbreviation">
		<rdfs:subPropertyOf rdf:resource="&fibo-fnd-utl-av;abbreviation"/>
		<rdfs:label>common abbreviation</rdfs:label>
		<rdfs:seeAlso rdf:resource="https://pe.usps.com/cpim/ftp/pubs/Pub28/pub28.pdf"/>
		<skos:definition>abbreviation or term that is typically used to refer to something</skos:definition>
	</owl:AnnotationProperty>
	
	<owl:ObjectProperty rdf:about="&fibo-fbc-fct-uspsaa;hasPostcode">
		<rdfs:subPropertyOf rdf:resource="&fibo-fnd-arr-arr;hasConstituent"/>
		<rdfs:label>has postcode</rdfs:label>
		<rdfs:range rdf:resource="&fibo-fbc-fct-uspsaa;Postcode"/>
		<skos:definition>indicates the zip or international postcode element of a delivery address</skos:definition>
	</owl:ObjectProperty>
	
	<owl:ObjectProperty rdf:about="&fibo-fbc-fct-uspsaa;hasUrbanization">
		<rdfs:subPropertyOf rdf:resource="&fibo-fnd-arr-arr;hasConstituent"/>
		<rdfs:label>has urbanization</rdfs:label>
		<rdfs:range rdf:resource="&fibo-fbc-fct-uspsaa;Urbanization"/>
		<skos:definition>indicates  area, sector, or development within a geographic area relevant to a delivery address</skos:definition>
	</owl:ObjectProperty>
	
	<owl:AnnotationProperty rdf:about="&fibo-fbc-fct-uspsaa;preferredAbbreviation">
		<rdfs:subPropertyOf rdf:resource="&fibo-fnd-utl-av;abbreviation"/>
		<rdfs:label>preferred abbreviation</rdfs:label>
		<rdfs:seeAlso rdf:resource="https://pe.usps.com/cpim/ftp/pubs/Pub28/pub28.pdf"/>
		<skos:definition>abbreviation or term that is recommended</skos:definition>
	</owl:AnnotationProperty>
	
	<owl:DatatypeProperty rdf:about="&fibo-fbc-fct-uspsaa;requiresSecondaryUnitRange">
		<rdfs:label>requires secondary unit range</rdfs:label>
		<rdfs:range rdf:resource="&xsd;boolean"/>
		<rdfs:seeAlso rdf:resource="https://pe.usps.com/cpim/ftp/pubs/Pub28/pub28.pdf"/>
		<skos:definition>if true, indicates that an additional qualifier is needed to complete the delivery point description, such as an apartment number</skos:definition>
		<fibo-fnd-utl-av:explanatoryNote>Note that in some cases, such as for lobby or office, if there are multiple secondary units then a range may be needed to differentiate between them, even if the range is not always required.</fibo-fnd-utl-av:explanatoryNote>
	</owl:DatatypeProperty>

</rdf:RDF>