<?xml version="1.0" encoding="UTF-8"?>
  
<!DOCTYPE rdf:RDF [
    <!ENTITY fibo-fnd-agr-ctr "http://spec.edmcouncil.org/fibo/red/fnd/agreements/contracts/">
    <!ENTITY fibo-uo-lat "http://spec.edmcouncil.org/fibo/red/uo/lattice/">
    <!ENTITY fibo-fnd-rl-prc "http://spec.edmcouncil.org/fibo/red/fnd/relative/party-role-context/">
    <!ENTITY fibo-rl-set "http://spec.edmcouncil.org/fibo/red/fnd/relative/set-membership/">
    <!ENTITY fibo-fnd-agrx-ext "http://spec.edmcouncil.org/fibo/red/fnd/agreements-ext/contracts-extensions/">
    <!ENTITY fibo-fnd-rel-rel "http://spec.edmcouncil.org/fibo/red/fnd/relations/relations/">
    <!ENTITY fibo-fnd-oac-own "http://spec.edmcouncil.org/fibo/red/fnd/ownership-and-control/ownership/">
    <!ENTITY fibo-fnd-utl-bt "http://spec.edmcouncil.org/fibo/red/fnd/utilities/business-facing-types/">
    <!ENTITY fibo-fnd-law-jur "http://spec.edmcouncil.org/fibo/red/fnd/law/jurisdictions/">
    <!ENTITY fibo-fnd-pty-pty "http://spec.edmcouncil.org/fibo/red/fnd/parties/parties/">
]>

<rdf:RDF xmlns:xsd="http://www.w3.org/2001/XMLSchema#"
         xmlns:sm="http://www.omg.org/techprocess/ab/SpecificationMetadata/"
         xmlns:xs="http://www.w3.org/2001/XMLSchema"
         xmlns:fibo-fnd-utl-av="http://www.omg.org/spec/EDMC-FIBO/FND/Utilities/AnnotationVocabulary/"
         xmlns:rdf="http://www.w3.org/1999/02/22-rdf-syntax-ns#"
         xmlns:rdfs="http://www.w3.org/2000/01/rdf-schema#"
         xmlns:owl="http://www.w3.org/2002/07/owl#"
         xmlns:skos="http://www.w3.org/2004/02/skos/core#"
         xmlns:dc="http://purl.org/dc/terms/"
         xml:base="http://spec.edmcouncil.org/fibo/red/fnd/agreements/contracts/">

   <owl:Ontology rdf:about="http://spec.edmcouncil.org/fibo/red/fnd/agreements/contracts/">
      <owl:imports rdf:resource="http://spec.edmcouncil.org/fibo/red/uo/lattice/"/>
      <owl:imports rdf:resource="http://spec.edmcouncil.org/fibo/red/fnd/relative/party-role-context/"/>
      <owl:imports rdf:resource="http://spec.edmcouncil.org/fibo/red/fnd/relative/set-membership/"/>
      <owl:imports rdf:resource="http://spec.edmcouncil.org/fibo/red/fnd/agreements-ext/contracts-extensions/"/>
      <owl:imports rdf:resource="http://spec.edmcouncil.org/fibo/red/fnd/relations/relations/"/>
      <owl:imports rdf:resource="http://spec.edmcouncil.org/fibo/red/fnd/ownership-and-control/ownership/"/>
      <owl:imports rdf:resource="http://spec.edmcouncil.org/fibo/red/fnd/utilities/business-facing-types/"/>
      <owl:imports rdf:resource="http://spec.edmcouncil.org/fibo/red/fnd/law/jurisdictions/"/>
      <owl:imports rdf:resource="http://spec.edmcouncil.org/fibo/red/fnd/parties/parties/"/>
   </owl:Ontology>


  <!--
    ///////////////////////////////////////////////////////////////////////////////////////
    //
    // Datatypes
    //
    ///////////////////////////////////////////////////////////////////////////////////////
    -->



  <!--
    ///////////////////////////////////////////////////////////////////////////////////////
    //
    // Object Properties
    //
    ///////////////////////////////////////////////////////////////////////////////////////
    -->


<owl:ObjectProperty rdf:about="&fibo-fnd-agr-ctr;bilateralContractHasPartyInRole">
      <rdfs:label>bilateral contract has party in role</rdfs:label>
      <rdfs:subPropertyOf rdf:resource="&fibo-fnd-pty-pty;hasPartyInRole"/>
      <rdfs:domain rdf:resource="&fibo-fnd-agr-ctr;BilateralContract"/>
      <rdfs:range rdf:resource="&fibo-fnd-pty-pty;PartyInRole"/>
   </owl:ObjectProperty>

   <owl:ObjectProperty rdf:about="&fibo-fnd-agr-ctr;contractTermsSetHasPart">
      <rdfs:label>contract terms set has part</rdfs:label>
      <skos:definition>A set of terms which forms part of the contract terms set. This may be a sub-clause, a clause or simply another definition of a set of terms at a smaller granularity than the set from which these are referred.</skos:definition>
      <rdfs:subPropertyOf rdf:resource="&fibo-fnd-rel-rel;hasPart"/>
      <rdfs:domain rdf:resource="&fibo-fnd-agr-ctr;ContractTermsSet"/>
      <rdfs:range rdf:resource="&fibo-fnd-agr-ctr;ContractTermsSet"/>
   </owl:ObjectProperty>

   <owl:ObjectProperty rdf:about="&fibo-fnd-agr-ctr;contractHasTerms">
      <rdfs:label>contract has terms</rdfs:label>
      <skos:definition>A set of terms that form part of the contract.</skos:definition>
      <rdfs:domain rdf:resource="&fibo-fnd-agr-ctr;Contract"/>
      <rdfs:range rdf:resource="&fibo-fnd-agr-ctr;ContractTermsSet"/>
   </owl:ObjectProperty>

   <owl:ObjectProperty rdf:about="&fibo-fnd-agr-ctr;contractHasPartyInRole">
      <rdfs:label>contract has party in role</rdfs:label>
      <rdfs:subPropertyOf rdf:resource="&fibo-fnd-pty-pty;hasPartyInRole"/>
      <rdfs:domain rdf:resource="&fibo-fnd-agr-ctr;Contract"/>
      <rdfs:range rdf:resource="&fibo-fnd-pty-pty;PartyInRole"/>
   </owl:ObjectProperty>

   <owl:ObjectProperty rdf:about="&fibo-fnd-agr-ctr;definesTermsFor">
      <rdfs:label>defines terms for</rdfs:label>
      <skos:definition>the contract sets out the terms for the something</skos:definition>
      <rdfs:domain rdf:resource="&fibo-fnd-agr-ctr;Contract"/>
      <rdfs:range rdf:resource="http://www.w3.org/2002/07/owl#Thing"/>
   </owl:ObjectProperty>

   <owl:ObjectProperty rdf:about="&fibo-fnd-agr-ctr;hasCounterparty">
      <rdfs:label>has counterparty</rdfs:label>
      <skos:definition>The second party to a contract. In the event that the contract identifies either party as being the principal, this is the other party to that contract.</skos:definition>
      <rdfs:subPropertyOf rdf:resource="&fibo-fnd-pty-pty;hasPartyInRole"/>
      <rdfs:subPropertyOf rdf:resource="&fibo-fnd-agrx-ext;hasParty"/>
      <rdfs:domain rdf:resource="&fibo-fnd-agr-ctr;Contract"/>
      <rdfs:range rdf:resource="&fibo-fnd-agr-ctr;ContractCounterparty"/>
   </owl:ObjectProperty>

   <owl:ObjectProperty rdf:about="&fibo-fnd-agr-ctr;hasGoverningJurisdiction">
      <rdfs:label>has governing jurisdiction</rdfs:label>
      <skos:definition>The jurisdiction under which the contract is governed, as agreed by both parties. In a written contract this is generally identified in a clause identified for example as Governing Law. This is the jurisdiction under which any disputes arising from the contract are to be resolved.</skos:definition>
      <rdfs:subPropertyOf rdf:resource="&fibo-fnd-rel-rel;isGoverneBy"/>
      <rdfs:domain rdf:resource="&fibo-fnd-agr-ctr;Contract"/>
      <rdfs:range rdf:resource="&fibo-fnd-law-jur;Jurisdiction"/>
   </owl:ObjectProperty>

   <owl:ObjectProperty rdf:about="&fibo-fnd-agr-ctr;hasNonBindingTerms">
      <rdfs:label>has non binding terms</rdfs:label>
      <skos:definition>Terms which are included in the contract but are not considered binding. A breach of such terms in the future would not be considered to be a breach of the contract.</skos:definition>
      <rdfs:subPropertyOf rdf:resource="&fibo-fnd-agr-ctr;contractHasTerms"/>
      <rdfs:domain rdf:resource="&fibo-fnd-agr-ctr;Contract"/>
      <rdfs:range rdf:resource="&fibo-fnd-agr-ctr;NonBindingTermsSet"/>
   </owl:ObjectProperty>

   <owl:ObjectProperty rdf:about="&fibo-fnd-agr-ctr;hasPrincipal">
      <rdfs:label>has principal</rdfs:label>
      <skos:definition>The main or principal party to the contract, if either party is identified as such.</skos:definition>
      <rdfs:subPropertyOf rdf:resource="&fibo-fnd-pty-pty;hasPartyInRole"/>
      <rdfs:subPropertyOf rdf:resource="&fibo-fnd-agrx-ext;hasParty"/>
      <rdfs:domain rdf:resource="&fibo-fnd-agr-ctr;Contract"/>
      <rdfs:range rdf:resource="&fibo-fnd-agr-ctr;ContractPrincipal"/>
   </owl:ObjectProperty>

   <owl:ObjectProperty rdf:about="&fibo-fnd-agr-ctr;hasThirdParty">
      <rdfs:label>has third party</rdfs:label>
      <skos:definition>A party which is not signatory to the party but has some role in the overall context defined by the contract.</skos:definition>
      <rdfs:subPropertyOf rdf:resource="&fibo-fnd-agrx-ext;hasParty"/>
      <rdfs:subPropertyOf rdf:resource="&fibo-fnd-pty-pty;hasPartyInRole"/>
      <rdfs:domain rdf:resource="&fibo-fnd-agr-ctr;Contract"/>
      <rdfs:range rdf:resource="&fibo-fnd-agr-ctr;ContractThirdParty"/>
   </owl:ObjectProperty>

   <owl:ObjectProperty rdf:about="&fibo-fnd-agr-ctr;heldBy">
      <rdfs:label>held by</rdfs:label>
      <skos:definition>The anonymous counterparty that holds the contract and may transfer the rights and obligations therein to another such holder.</skos:definition>
      <rdfs:subPropertyOf rdf:resource="&fibo-fnd-agr-ctr;hasCounterparty"/>
      <rdfs:domain rdf:resource="&fibo-fnd-agr-ctr;TransferableContract"/>
      <rdfs:range rdf:resource="&fibo-fnd-agr-ctr;TransferableContractHolder"/>
   </owl:ObjectProperty>

   <owl:ObjectProperty rdf:about="&fibo-fnd-agr-ctr;writtenBy">
      <rdfs:label>written by</rdfs:label>
      <skos:definition>The party by whom the transferable contract has been written.</skos:definition>
      <rdfs:subPropertyOf rdf:resource="&fibo-fnd-agr-ctr;hasPrincipal"/>
      <rdfs:domain rdf:resource="&fibo-fnd-agr-ctr;TransferableContract"/>
      <rdfs:range rdf:resource="&fibo-fnd-agr-ctr;ContractOriginator"/>
   </owl:ObjectProperty>

   <owl:ObjectProperty rdf:about="&fibo-fnd-agr-ctr;supersedes">
      <rdfs:label>supersedes</rdfs:label>
      <skos:definition>The or any earlier contract which this written contract supersedes, whether that earlier contract is written or verbal or implied.</skos:definition>
      <rdfs:domain rdf:resource="&fibo-fnd-agr-ctr;WrittenContract"/>
      <rdfs:range rdf:resource="&fibo-fnd-agr-ctr;Contract"/>
   </owl:ObjectProperty>


  <!--
    ///////////////////////////////////////////////////////////////////////////////////////
    //
    // Data Properties
    //
    ///////////////////////////////////////////////////////////////////////////////////////
    -->


<owl:DatatypeProperty rdf:about="&fibo-fnd-agr-ctr;hasEffectiveDate">
      <rdfs:label>has effective date</rdfs:label>
      <skos:definition>The date upon which the contract comes into force.</skos:definition>
      <rdfs:range rdf:resource="http://www.w3.org/2001/XMLSchema#date"/>
   </owl:DatatypeProperty>

   <owl:DatatypeProperty rdf:about="&fibo-fnd-agr-ctr;isAssignable">
      <rdfs:label>is assignable</rdfs:label>
      <skos:definition>Whether the contracts and the rights thereunder may be assigned by one of the signatories to some other party. Editorial Note: This is the basis on which transferable contracts such as financial securities and software licences may be bought and sold on some market, and also the basis on which a bilateral contract such as an over the counter derivative may be novated so that a new party becomes one of the parties.</skos:definition>
      <rdfs:range rdf:resource="&fibo-fnd-utl-bt;yesOrNo"/>
   </owl:DatatypeProperty>


  <!--
    ///////////////////////////////////////////////////////////////////////////////////////
    //
    // Annotation Properties
    //
    ///////////////////////////////////////////////////////////////////////////////////////
    -->



  <!--
    ///////////////////////////////////////////////////////////////////////////////////////
    //
    // Classes
    //
    ///////////////////////////////////////////////////////////////////////////////////////
    -->


<owl:Class rdf:about="&fibo-fnd-agr-ctr;ConditionsPrecedent">
      <rdfs:label>conditions precedent</rdfs:label>
      <skos:definition>Conditions precedent on some obligation. These are conditions which would alter the Obligation as it is otherwise stated.</skos:definition>
      <rdfs:subClassOf rdf:resource="&fibo-fnd-agr-ctr;ContractTermsSet"/>
   </owl:Class>

   <owl:Class rdf:about="&fibo-fnd-agr-ctr;Contract">
      <rdfs:label>contract</rdfs:label>
      <rdfs:subClassOf rdf:resource="&fibo-uo-lat;ContinuantThing"/>
      <rdfs:subClassOf rdf:resource="&fibo-fnd-rl-prc;RelationshipContext"/>
      <rdfs:subClassOf rdf:resource="&fibo-uo-lat;Concrete"/>
   </owl:Class>

   <owl:Class rdf:about="&fibo-fnd-agr-ctr;ContractCounterparty">
      <rdfs:label>contract counterparty</rdfs:label>
      <rdfs:subClassOf rdf:resource="&fibo-fnd-pty-pty;PartyInRole"/>
      <rdfs:subClassOf rdf:resource="&fibo-fnd-agrx-ext;ContractParty"/>
   </owl:Class>

   <owl:Class rdf:about="&fibo-fnd-agr-ctr;ContractPrincipal">
      <rdfs:label>contract principal</rdfs:label>
      <skos:definition>The party identified as being the principal or first party to a contract, in the event that the contract distinguishes either party as being the principal.</skos:definition>
   </owl:Class>

   <owl:Class rdf:about="&fibo-fnd-agr-ctr;ContractTermsSet">
      <rdfs:label>contract terms set</rdfs:label>
      <rdfs:subClassOf rdf:resource="&fibo-fnd-agr-ctr;ContractualElement"/>
      <rdfs:subClassOf rdf:resource="&fibo-rl-set;Set"/>
   </owl:Class>

   <owl:Class rdf:about="&fibo-fnd-agr-ctr;ContractThirdParty">
      <rdfs:label>contract third party</rdfs:label>
      <skos:definition>A party which is identified in a contract but which is not itself party to that contract.</skos:definition>
   </owl:Class>

   <owl:Class rdf:about="&fibo-fnd-agr-ctr;ContractualDefinition">
      <rdfs:label>contractual definition</rdfs:label>
      <skos:definition>The definition of something in some contract or other legal instrument.</skos:definition>
   </owl:Class>

   <owl:Class rdf:about="&fibo-fnd-agr-ctr;ContractualElement">
      <rdfs:label>contractual element</rdfs:label>
      <skos:definition>Anything which relates to contracts.</skos:definition>
   </owl:Class>

   <owl:Class rdf:about="&fibo-fnd-agr-ctr;ContractualRelationship">
      <rdfs:label>contractual relationship</rdfs:label>
      <skos:definition>A relationship in which two or more parties have some contractual obligations or extend some rights under a contract, to one another.</skos:definition>
   </owl:Class>

   <owl:Class rdf:about="&fibo-fnd-agr-ctr;NonBindingTermsSet">
      <rdfs:label>non binding terms set</rdfs:label>
      <skos:definition>Terms which do not have binding legal standing on the Issuer or Holder.</skos:definition>
   </owl:Class>

   <owl:Class rdf:about="&fibo-fnd-agr-ctr;PromissoryNote">
      <rdfs:label>promissory note</rdfs:label>
      <skos:definition>A promise by the issuer of the note, of some good or benefit to the holder.</skos:definition>
      <rdfs:subClassOf rdf:resource="&fibo-fnd-agr-ctr;WrittenContract"/>
   </owl:Class>

   <owl:Class rdf:about="&fibo-fnd-agr-ctr;TransferableContractHolder">
      <rdfs:label>transferable contract holder</rdfs:label>
      <skos:definition>The party which holds a transferable contract and enjoys the benefits defined in that contract while they hold it.</skos:definition>
      <rdfs:subClassOf rdf:resource="&fibo-fnd-agr-ctr;ContractCounterparty"/>
      <rdfs:subClassOf rdf:resource="&fibo-fnd-oac-own;Owner"/>
   </owl:Class>

   <owl:Class rdf:about="&fibo-fnd-agr-ctr;BilateralContract">
      <rdfs:label>bilateral contract</rdfs:label>
      <skos:definition>A contract between two specific named parties. The rights and obligations pertaining to either party cannot be transferred to another party without prior written permission or a change to the contract itself.</skos:definition>
      <rdfs:subClassOf rdf:resource="&fibo-fnd-agr-ctr;Contract"/>
   </owl:Class>

   <owl:Class rdf:about="&fibo-fnd-agr-ctr;TransferableContract">
      <rdfs:label>transferable contract</rdfs:label>
   </owl:Class>

   <owl:Class rdf:about="&fibo-fnd-agr-ctr;VerbalContract">
      <rdfs:label>verbal contract</rdfs:label>
   </owl:Class>

   <owl:Class rdf:about="&fibo-fnd-agr-ctr;ContractOriginator">
      <rdfs:label>contract originator</rdfs:label>
      <skos:definition>The party which originates the transferable contract and acts as the Principal in that contract.</skos:definition>
      <rdfs:subClassOf rdf:resource="&fibo-fnd-agr-ctr;ContractPrincipal"/>
   </owl:Class>

   <owl:Class rdf:about="&fibo-fnd-agr-ctr;WrittenContract">
      <rdfs:label>written contract</rdfs:label>
      <skos:definition>A formal Contract which is written and signed by both parties thereto.</skos:definition>
   </owl:Class>


  <!--
    ///////////////////////////////////////////////////////////////////////////////////////
    //
    // Individuals
    //
    ///////////////////////////////////////////////////////////////////////////////////////
    -->


</rdf:RDF>