<?xml version="1.0" encoding="UTF-8"?>
  
<!DOCTYPE rdf:RDF [
    <!ENTITY fibo-fnd-aap-ppl "http://spec.edmcouncil.org/fibo/red/fnd/agents-and-people/people/">
    <!ENTITY fibo-fnd-aap-agt "http://spec.edmcouncil.org/fibo/red/fnd/agents-and-people/agents/">
    <!ENTITY fibo-fnd-plc-cty "http://spec.edmcouncil.org/fibo/red/fnd/places/countries/">
    <!ENTITY fibo-fnd-utl-bt "http://spec.edmcouncil.org/fibo/red/fnd/utilities/business-facing-types/">
]>

<rdf:RDF xmlns:xsd="http://www.w3.org/2001/XMLSchema#"
         xmlns:sm="http://www.omg.org/techprocess/ab/SpecificationMetadata/"
         xmlns:xs="http://www.w3.org/2001/XMLSchema"
         xmlns:fibo-fnd-utl-av="http://www.omg.org/spec/EDMC-FIBO/FND/Utilities/AnnotationVocabulary/"
         xmlns:rdf="http://www.w3.org/1999/02/22-rdf-syntax-ns#"
         xmlns:rdfs="http://www.w3.org/2000/01/rdf-schema#"
         xmlns:owl="http://www.w3.org/2002/07/owl#"
         xmlns:skos="http://www.w3.org/2004/02/skos/core#"
         xmlns:dc="http://purl.org/dc/terms/"
         xml:base="http://spec.edmcouncil.org/fibo/red/fnd/agents-and-people/people/">

   <owl:Ontology rdf:about="http://spec.edmcouncil.org/fibo/red/fnd/agents-and-people/people/">
      <owl:imports rdf:resource="http://spec.edmcouncil.org/fibo/red/fnd/agents-and-people/agents/"/>
      <owl:imports rdf:resource="http://spec.edmcouncil.org/fibo/red/fnd/places/countries/"/>
      <owl:imports rdf:resource="http://spec.edmcouncil.org/fibo/red/fnd/utilities/business-facing-types/"/>
   </owl:Ontology>


  <!--
    ///////////////////////////////////////////////////////////////////////////////////////
    //
    // Datatypes
    //
    ///////////////////////////////////////////////////////////////////////////////////////
    -->


<rdfs:Datatype rdf:about="&fibo-fnd-aap-ppl;Gender">
      <skos:definition>Selection of possible Genders which may be attributed to a person.</skos:definition>
      <owl:equivalentClass>
         <rdfs:Datatype>
            <owl:oneOf>
               <rdf:Description>
                  <rdf:first rdf:datatype="http://www.w3.org/2001/XMLSchema#string">Female</rdf:first>
                  <rdf:rest>
                     <rdf:Description>
                        <rdf:first rdf:datatype="http://www.w3.org/2001/XMLSchema#string">Unspecified</rdf:first>
                        <rdf:rest>
                           <rdf:Description>
                              <rdf:first rdf:datatype="http://www.w3.org/2001/XMLSchema#string">Male</rdf:first>
                              <rdf:rest rdf:resource="http://www.w3.org/1999/02/22-rdf-syntax-ns#nil"/>
                           </rdf:Description>
                        </rdf:rest>
                     </rdf:Description>
                  </rdf:rest>
               </rdf:Description>
            </owl:oneOf>
         </rdfs:Datatype>
      </owl:equivalentClass>
   </rdfs:Datatype>


  <!--
    ///////////////////////////////////////////////////////////////////////////////////////
    //
    // Object Properties
    //
    ///////////////////////////////////////////////////////////////////////////////////////
    -->


<owl:ObjectProperty rdf:about="&fibo-fnd-aap-ppl;citizenship">
      <rdfs:label>citizenship</rdfs:label>
      <skos:definition>A country of and by which the person is formally recognized as a citizen.</skos:definition>
      <rdfs:domain rdf:resource="&fibo-fnd-aap-ppl;Person"/>
      <rdfs:range rdf:resource="&fibo-fnd-plc-cty;Country"/>
   </owl:ObjectProperty>


  <!--
    ///////////////////////////////////////////////////////////////////////////////////////
    //
    // Data Properties
    //
    ///////////////////////////////////////////////////////////////////////////////////////
    -->


<owl:DatatypeProperty rdf:about="&fibo-fnd-aap-ppl;dateOfBirth">
      <rdfs:label>date of birth</rdfs:label>
      <skos:definition>Date on which the person was born as registered on a birth certificate if available.</skos:definition>
      <rdfs:range rdf:resource="http://www.w3.org/2001/XMLSchema#date"/>
   </owl:DatatypeProperty>

   <owl:DatatypeProperty rdf:about="&fibo-fnd-aap-ppl;familyName">
      <rdfs:label>family name</rdfs:label>
      <rdfs:range rdf:resource="&fibo-fnd-utl-bt;text"/>
   </owl:DatatypeProperty>

   <owl:DatatypeProperty rdf:about="&fibo-fnd-aap-ppl;fullLegalName">
      <rdfs:label>full legal name</rdfs:label>
      <rdfs:range rdf:resource="&fibo-fnd-utl-bt;text"/>
   </owl:DatatypeProperty>

   <owl:DatatypeProperty rdf:about="&fibo-fnd-aap-ppl;gender">
      <rdfs:label>gender</rdfs:label>
      <skos:definition>The gender of the person as defined by that person for the purposes of identifying or describing themselves, for example to an institution with which they interact.</skos:definition>
      <rdfs:range rdf:resource="&fibo-fnd-aap-ppl;Gender"/>
   </owl:DatatypeProperty>

   <owl:DatatypeProperty rdf:about="&fibo-fnd-aap-ppl;givenName">
      <rdfs:label>given name</rdfs:label>
      <rdfs:range rdf:resource="&fibo-fnd-utl-bt;text"/>
   </owl:DatatypeProperty>


  <!--
    ///////////////////////////////////////////////////////////////////////////////////////
    //
    // Annotation Properties
    //
    ///////////////////////////////////////////////////////////////////////////////////////
    -->



  <!--
    ///////////////////////////////////////////////////////////////////////////////////////
    //
    // Classes
    //
    ///////////////////////////////////////////////////////////////////////////////////////
    -->


<owl:Class rdf:about="&fibo-fnd-aap-ppl;Adult">
      <rdfs:label>adult</rdfs:label>
      <skos:definition>Biologically, an adult is a human being or other organism that is of reproductive age (sexual maturity). In human context, the term adult additionally has meanings associated with social and legal concepts; for example, a legal adult is a legal concept for a person who has attained the age of majority and is therefore regarded as independent, self-sufficient, and responsible (contrast with minor). In addition, human adulthood encompasses psychological adult development.</skos:definition>
      <rdfs:subClassOf rdf:resource="&fibo-fnd-aap-ppl;Person"/>
   </owl:Class>

   <owl:Class rdf:about="&fibo-fnd-aap-ppl;EmancipatedMinor">
      <rdfs:label>emancipated minor</rdfs:label>
      <skos:definition>An emancipated minor is a minor who is allowed to conduct a business or any other occupation on his or her own behalf or for their own account outside the influence of a parent or guardian. The minor will then have full contractual capacity to conclude contracts with regard to the business. Whether parental consent is needed to achieve emancipated status varies from case to case. In some cases, court permission is necessary. Protocols vary by jurisdiction.</skos:definition>
      <rdfs:subClassOf rdf:resource="&fibo-fnd-aap-ppl;Minor"/>
   </owl:Class>

   <owl:Class rdf:about="&fibo-fnd-aap-ppl;IncapacitatedAdult">
      <rdfs:label>incapacitated adult</rdfs:label>
      <skos:definition>Individuals may have an inherent physical condition which prevents them from achieving the normal levels of performance expected from persons of comparable age, or their inability to match current levels of performance may be caused by contracting an illness. Whatever the cause, if the resulting condition is such that individuals cannot care for themselves, or may act in ways that are against their interests, those persons are vulnerable through dependency and require the protection of the state against the risks of abuse or exploitation. Hence, any agreements that were made are voidable, and a court may declare that person a ward of the state and grant power of attorney to an appointed legal guardian.</skos:definition>
      <rdfs:subClassOf rdf:resource="&fibo-fnd-aap-ppl;Adult"/>
   </owl:Class>

   <owl:Class rdf:about="&fibo-fnd-aap-ppl;Minor">
      <rdfs:label>minor</rdfs:label>
   </owl:Class>

   <owl:Class rdf:about="&fibo-fnd-aap-ppl;Person">
      <rdfs:label>person</rdfs:label>
      <skos:definition>A person; any member of the species homo sapiens.</skos:definition>
      <rdfs:subClassOf rdf:resource="&fibo-fnd-aap-agt;AutonomousAgent"/>
   </owl:Class>


  <!--
    ///////////////////////////////////////////////////////////////////////////////////////
    //
    // Individuals
    //
    ///////////////////////////////////////////////////////////////////////////////////////
    -->


</rdf:RDF>