<?xml version="1.0" encoding="UTF-8"?>
  
<!DOCTYPE rdf:RDF [
    <!ENTITY fibo-loan-loan-bt "http://spec.edmcouncil.org/fibo/red/loan/loans/loan-basic-terms/">
    <!ENTITY fibo-fnd-agrx-ext "http://spec.edmcouncil.org/fibo/red/fnd/agreements-ext/contracts-extensions/">
    <!ENTITY fibo-md-tmp-tmp "http://spec.edmcouncil.org/fibo/red/md/temporal-core/temporal-concepts/">
    <!ENTITY fibo-fnd-info-info "http://spec.edmcouncil.org/fibo/red/fnd/information/info-core/">
    <!ENTITY fibo-fnd-info-ids "http://spec.edmcouncil.org/fibo/red/fnd/information/identifiers/">
    <!ENTITY fibo-fnd-acc-dbt "http://spec.edmcouncil.org/fibo/red/fnd/accounting/debt-terms/">
    <!ENTITY fibo-fnd-pty-pty "http://spec.edmcouncil.org/fibo/red/fnd/parties/parties/">
    <!ENTITY fibo-fnd-agr-ctr "http://spec.edmcouncil.org/fibo/red/fnd/agreements/contracts/">
    <!ENTITY fibo-fnd-acc-cur "http://spec.edmcouncil.org/fibo/red/fnd/accounting/currency-amount/">
    <!ENTITY fibo-loan-loan-par "http://spec.edmcouncil.org/fibo/red/loan/loans/loans-parties/">
    <!ENTITY fibo-fnd-tim-tim "http://spec.edmcouncil.org/fibo/red/fnd/date-time/date-time/">
    <!ENTITY fibo-fnd-utl-bt "http://spec.edmcouncil.org/fibo/red/fnd/utilities/business-facing-types/">
    <!ENTITY fibo-be-le-lp "http://spec.edmcouncil.org/fibo/red/be/legal-entities/legal-persons/">
    <!ENTITY fibo-ind-ind-ind "http://spec.edmcouncil.org/fibo/red/ind/indicators/indicators/">
    <!ENTITY fibo-ind-ir-ir "http://spec.edmcouncil.org/fibo/red/ind/interest-rates/interest-rates/">
    <!ENTITY fibo-loan-loan-loan "http://spec.edmcouncil.org/fibo/red/loan/loans/loans-general/">
    <!ENTITY fibo-loan-tmp-ph "http://spec.edmcouncil.org/fibo/red/loan/loans-temporal/loan-phases/">
    <!ENTITY fibo-fnd-agrx-cst "http://spec.edmcouncil.org/fibo/red/fnd/agreements-ext/contractual-constructs/">
]>

<rdf:RDF xmlns:xsd="http://www.w3.org/2001/XMLSchema#"
         xmlns:sm="http://www.omg.org/techprocess/ab/SpecificationMetadata/"
         xmlns:xs="http://www.w3.org/2001/XMLSchema"
         xmlns:fibo-fnd-utl-av="http://www.omg.org/spec/EDMC-FIBO/FND/Utilities/AnnotationVocabulary/"
         xmlns:rdf="http://www.w3.org/1999/02/22-rdf-syntax-ns#"
         xmlns:rdfs="http://www.w3.org/2000/01/rdf-schema#"
         xmlns:owl="http://www.w3.org/2002/07/owl#"
         xmlns:skos="http://www.w3.org/2004/02/skos/core#"
         xmlns:dc="http://purl.org/dc/terms/"
         xml:base="http://spec.edmcouncil.org/fibo/red/loan/loans/loan-basic-terms/">

   <owl:Ontology rdf:about="http://spec.edmcouncil.org/fibo/red/loan/loans/loan-basic-terms/">
      <owl:imports rdf:resource="http://spec.edmcouncil.org/fibo/red/fnd/agreements-ext/contracts-extensions/"/>
      <owl:imports rdf:resource="http://spec.edmcouncil.org/fibo/red/md/temporal-core/temporal-concepts/"/>
      <owl:imports rdf:resource="http://spec.edmcouncil.org/fibo/red/fnd/information/info-core/"/>
      <owl:imports rdf:resource="http://spec.edmcouncil.org/fibo/red/fnd/information/identifiers/"/>
      <owl:imports rdf:resource="http://spec.edmcouncil.org/fibo/red/fnd/accounting/debt-terms/"/>
      <owl:imports rdf:resource="http://spec.edmcouncil.org/fibo/red/fnd/parties/parties/"/>
      <owl:imports rdf:resource="http://spec.edmcouncil.org/fibo/red/fnd/agreements/contracts/"/>
      <owl:imports rdf:resource="http://spec.edmcouncil.org/fibo/red/fnd/accounting/currency-amount/"/>
      <owl:imports rdf:resource="http://spec.edmcouncil.org/fibo/red/loan/loans/loans-parties/"/>
      <owl:imports rdf:resource="http://spec.edmcouncil.org/fibo/red/fnd/date-time/date-time/"/>
      <owl:imports rdf:resource="http://spec.edmcouncil.org/fibo/red/fnd/utilities/business-facing-types/"/>
      <owl:imports rdf:resource="http://spec.edmcouncil.org/fibo/red/be/legal-entities/legal-persons/"/>
      <owl:imports rdf:resource="http://spec.edmcouncil.org/fibo/red/ind/indicators/indicators/"/>
      <owl:imports rdf:resource="http://spec.edmcouncil.org/fibo/red/ind/interest-rates/interest-rates/"/>
      <owl:imports rdf:resource="http://spec.edmcouncil.org/fibo/red/loan/loans/loans-general/"/>
      <owl:imports rdf:resource="http://spec.edmcouncil.org/fibo/red/loan/loans-temporal/loan-phases/"/>
      <owl:imports rdf:resource="http://spec.edmcouncil.org/fibo/red/fnd/agreements-ext/contractual-constructs/"/>
   </owl:Ontology>


  <!--
    ///////////////////////////////////////////////////////////////////////////////////////
    //
    // Datatypes
    //
    ///////////////////////////////////////////////////////////////////////////////////////
    -->


<rdfs:Datatype rdf:about="&fibo-loan-loan-bt;LoanPenaltyInterestApplicationSelection">
      <skos:definition>Selection of types of balance to which pre-payment interest penalties may be applied.</skos:definition>
      <owl:equivalentClass>
         <rdfs:Datatype>
            <owl:oneOf>
               <rdf:Description>
                  <rdf:first rdf:datatype="http://www.w3.org/2001/XMLSchema#string">Current Principal Balance</rdf:first>
                  <rdf:rest>
                     <rdf:Description>
                        <rdf:first rdf:datatype="http://www.w3.org/2001/XMLSchema#string">Original Balance</rdf:first>
                        <rdf:rest>
                           <rdf:Description>
                              <rdf:first rdf:datatype="http://www.w3.org/2001/XMLSchema#string">Curtailment Amount</rdf:first>
                              <rdf:rest rdf:resource="http://www.w3.org/1999/02/22-rdf-syntax-ns#nil"/>
                           </rdf:Description>
                        </rdf:rest>
                     </rdf:Description>
                  </rdf:rest>
               </rdf:Description>
            </owl:oneOf>
         </rdfs:Datatype>
      </owl:equivalentClass>
   </rdfs:Datatype>

   <rdfs:Datatype rdf:about="&fibo-loan-loan-bt;LoanTypeSelection">
      <skos:definition>A selection of different types of loan purpose, being the purpose for which and manner in which loan (credit) draw-down amounts are to be used. This shows the purpose for which credit is to be used, and implies certain kinds of fact that relate to that specific type of loan e.g. mortgages. These are also identified as tranche types in tranches of a credit facility.</skos:definition>
      <owl:equivalentClass>
         <rdfs:Datatype>
            <owl:oneOf>
               <rdf:Description>
                  <rdf:first rdf:datatype="http://www.w3.org/2001/XMLSchema#string">Auto Loan</rdf:first>
                  <rdf:rest>
                     <rdf:Description>
                        <rdf:first rdf:datatype="http://www.w3.org/2001/XMLSchema#string">Bridging Loan</rdf:first>
                        <rdf:rest>
                           <rdf:Description>
                              <rdf:first rdf:datatype="http://www.w3.org/2001/XMLSchema#string">Construction</rdf:first>
                              <rdf:rest>
                                 <rdf:Description>
                                    <rdf:first rdf:datatype="http://www.w3.org/2001/XMLSchema#string">Credit Card Receivable</rdf:first>
                                    <rdf:rest>
                                       <rdf:Description>
                                          <rdf:first rdf:datatype="http://www.w3.org/2001/XMLSchema#string">Drawing Rights</rdf:first>
                                          <rdf:rest>
                                             <rdf:Description>
                                                <rdf:first rdf:datatype="http://www.w3.org/2001/XMLSchema#string">Working Capital</rdf:first>
                                                <rdf:rest>
                                                   <rdf:Description>
                                                      <rdf:first rdf:datatype="http://www.w3.org/2001/XMLSchema#string">Motorhome Loan</rdf:first>
                                                      <rdf:rest>
                                                         <rdf:Description>
                                                            <rdf:first rdf:datatype="http://www.w3.org/2001/XMLSchema#string">Ordinary Loan</rdf:first>
                                                            <rdf:rest>
                                                               <rdf:Description>
                                                                  <rdf:first rdf:datatype="http://www.w3.org/2001/XMLSchema#string">Overdraft Facility</rdf:first>
                                                                  <rdf:rest>
                                                                     <rdf:Description>
                                                                        <rdf:first rdf:datatype="http://www.w3.org/2001/XMLSchema#string">Residential Houseboat Loan</rdf:first>
                                                                        <rdf:rest>
                                                                           <rdf:Description>
                                                                              <rdf:first rdf:datatype="http://www.w3.org/2001/XMLSchema#string">Student Loan</rdf:first>
                                                                              <rdf:rest>
                                                                                 <rdf:Description>
                                                                                    <rdf:first rdf:datatype="http://www.w3.org/2001/XMLSchema#string">Home Equity Loan</rdf:first>
                                                                                    <rdf:rest rdf:resource="http://www.w3.org/1999/02/22-rdf-syntax-ns#nil"/>
                                                                                 </rdf:Description>
                                                                              </rdf:rest>
                                                                           </rdf:Description>
                                                                        </rdf:rest>
                                                                     </rdf:Description>
                                                                  </rdf:rest>
                                                               </rdf:Description>
                                                            </rdf:rest>
                                                         </rdf:Description>
                                                      </rdf:rest>
                                                   </rdf:Description>
                                                </rdf:rest>
                                             </rdf:Description>
                                          </rdf:rest>
                                       </rdf:Description>
                                    </rdf:rest>
                                 </rdf:Description>
                              </rdf:rest>
                           </rdf:Description>
                        </rdf:rest>
                     </rdf:Description>
                  </rdf:rest>
               </rdf:Description>
            </owl:oneOf>
         </rdfs:Datatype>
      </owl:equivalentClass>
   </rdfs:Datatype>


  <!--
    ///////////////////////////////////////////////////////////////////////////////////////
    //
    // Object Properties
    //
    ///////////////////////////////////////////////////////////////////////////////////////
    -->


<owl:ObjectProperty rdf:about="&fibo-loan-loan-bt;acceptedBy">
      <rdfs:label>accepted by</rdfs:label>
      <rdfs:domain rdf:resource="&fibo-loan-loan-bt;LoanBorrowerCommitment"/>
      <rdfs:range rdf:resource="&fibo-be-le-lp;LegalPerson"/>
      <owl:inverseOf rdf:resource="&fibo-loan-loan-bt;accepts"/>
   </owl:ObjectProperty>

   <owl:ObjectProperty rdf:about="&fibo-loan-loan-bt;accepts">
      <rdfs:label>accepts</rdfs:label>
      <rdfs:domain rdf:resource="&fibo-be-le-lp;LegalPerson"/>
      <rdfs:range rdf:resource="&fibo-loan-loan-bt;LoanBorrowerCommitment"/>
   </owl:ObjectProperty>

   <owl:ObjectProperty rdf:about="&fibo-loan-loan-bt;loanDenominationCurrency">
      <rdfs:label>loan denomination currency</rdfs:label>
      <skos:definition>The currency in which the loan is denominated.</skos:definition>
      <rdfs:domain rdf:resource="&fibo-loan-loan-bt;Loan"/>
      <rdfs:range rdf:resource="&fibo-fnd-acc-cur;Currency"/>
   </owl:ObjectProperty>

   <owl:ObjectProperty rdf:about="&fibo-loan-loan-bt;loanIdentifier">
      <rdfs:label>loan identifier</rdfs:label>
      <skos:definition>Unique identifier for the loan. Further notes: This is an information construct. It is internal rather than a publicly available ID (like ISIN) but is included since it is a fundamental "fact" about the loan regardless of the fact that it exists only as a data model construct. The loan ID should not change through the life of the transaction. Data model note (not applicable to semantic model): If the original loan ID cannot be maintained in this field enter the original ID followed by the new ID, comma delimited</skos:definition>
      <rdfs:domain rdf:resource="&fibo-loan-loan-bt;Loan"/>
      <rdfs:range rdf:resource="&fibo-loan-loan-bt;LoanIdentifier"/>
   </owl:ObjectProperty>

   <owl:ObjectProperty rdf:about="&fibo-loan-loan-bt;loanSubsidyAmount">
      <rdfs:label>loan subsidy amount</rdfs:label>
      <skos:definition>Loan Subsidy Received - Amount of subsidy received from government by borrower.</skos:definition>
      <rdfs:domain rdf:resource="&fibo-loan-loan-bt;Loan"/>
      <rdfs:range rdf:resource="&fibo-fnd-acc-cur;MoneyAmount"/>
   </owl:ObjectProperty>

   <owl:ObjectProperty rdf:about="&fibo-loan-loan-bt;maturity">
      <rdfs:label>maturity</rdfs:label>
      <skos:definition>The period of time before which the loan is to be repaid or the credit facility expires, if any.</skos:definition>
      <rdfs:domain rdf:resource="&fibo-loan-loan-bt;Loan"/>
      <rdfs:range rdf:resource="&fibo-md-tmp-tmp;TimedDurationSpecification"/>
   </owl:ObjectProperty>

   <owl:ObjectProperty rdf:about="&fibo-loan-loan-bt;acceptedBy.1">
      <rdfs:label>accepted by</rdfs:label>
      <rdfs:subPropertyOf rdf:resource="&fibo-loan-loan-bt;acceptedBy"/>
      <rdfs:domain rdf:resource="&fibo-loan-loan-bt;LoanBorrowerCommitment"/>
      <rdfs:range rdf:resource="&fibo-loan-loan-par;LoanBorrower"/>
   </owl:ObjectProperty>

   <owl:ObjectProperty rdf:about="&fibo-loan-loan-bt;loanAmortizationPeriod">
      <rdfs:label>loan amortization period</rdfs:label>
      <skos:definition>Loan Term, that is the original contractual term of the loan, in months.</skos:definition>
      <rdfs:domain rdf:resource="&fibo-loan-loan-bt;LoanContract"/>
      <rdfs:range rdf:resource="&fibo-fnd-tim-tim;DatePeriod"/>
   </owl:ObjectProperty>

   <owl:ObjectProperty rdf:about="&fibo-loan-loan-bt;loanMaximumAllowedBalance">
      <rdfs:label>loan maximum allowed balance</rdfs:label>
      <skos:definition>Maximum balance - For loans with flexible re-draw facilities, the maximum loan amount that could potentially be outstanding</skos:definition>
      <rdfs:domain rdf:resource="&fibo-loan-loan-bt;LoanContract"/>
      <rdfs:range rdf:resource="&fibo-fnd-acc-cur;MoneyAmount"/>
   </owl:ObjectProperty>

   <owl:ObjectProperty rdf:about="&fibo-loan-loan-bt;loanOriginalAdvanceAmount">
      <rdfs:label>loan original advance amount</rdfs:label>
      <skos:definition>The Original Balance of the loan, that is the amount advanced under this loan. Further notes: PoC workings: Original balance (inclusive of fees)</skos:definition>
      <rdfs:domain rdf:resource="&fibo-loan-loan-bt;LoanContract"/>
      <rdfs:range rdf:resource="&fibo-fnd-acc-cur;MonetaryAmount"/>
   </owl:ObjectProperty>

   <owl:ObjectProperty rdf:about="&fibo-loan-loan-bt;loanPaymentFrequency">
      <rdfs:label>loan payment frequency</rdfs:label>
      <skos:definition>Payment Frequency - Frequency of payments due, i.e. number of months between payments. Further notes: This is defined as a frequency, i.e. the reciprocal of a period of time. Corresponding Data model entries: Monthly Quarterly Semi annually Annual Bullet Other (to provide details, if applicable) No data Note that not all of these correspond to frequency. Therefore one possibility is that this term is not present. Arrangements such as bullet payments are part of the principal and interest payment terms. This term is retained as a fact about the Loan Contract because the lender may be contractually obliged to make payments with this regularity, which combine interest, principal and other amounts (Tax, ESCROW etc.).</skos:definition>
      <rdfs:domain rdf:resource="&fibo-loan-loan-bt;LoanContract"/>
      <rdfs:range rdf:resource="&fibo-fnd-tim-tim;Frequency"/>
   </owl:ObjectProperty>

   <owl:ObjectProperty rdf:about="&fibo-loan-loan-bt;loanPeriodicPayment">
      <rdfs:label>loan periodic payment</rdfs:label>
      <skos:definition>Periodic contractual payment due (the payment due if there are no other payment arrangements in force)</skos:definition>
      <rdfs:domain rdf:resource="&fibo-loan-loan-bt;LoanContract"/>
      <rdfs:range rdf:resource="&fibo-fnd-acc-cur;MoneyAmount"/>
   </owl:ObjectProperty>

   <owl:ObjectProperty rdf:about="&fibo-loan-loan-bt;loanRetainedAmount">
      <rdfs:label>loan retained amount</rdfs:label>
      <skos:definition>Retained amount, this is an amount the Issuer will be obliged to fund to the borrower at a later date, for example construction deposit.</skos:definition>
      <rdfs:domain rdf:resource="&fibo-loan-loan-bt;LoanContract"/>
      <rdfs:range rdf:resource="&fibo-fnd-acc-cur;MoneyAmount"/>
   </owl:ObjectProperty>

   <owl:ObjectProperty rdf:about="&fibo-loan-loan-bt;establishes">
      <rdfs:label>establishes</rdfs:label>
      <rdfs:subPropertyOf rdf:resource="&fibo-fnd-agrx-cst;mandates"/>
      <rdfs:domain rdf:resource="&fibo-loan-loan-bt;LoanContract"/>
      <rdfs:range rdf:resource="&fibo-loan-loan-bt;LoanInterestPaymentCommitment"/>
   </owl:ObjectProperty>

   <owl:ObjectProperty rdf:about="&fibo-loan-loan-bt;establishes.1">
      <rdfs:label>establishes</rdfs:label>
      <rdfs:subPropertyOf rdf:resource="&fibo-fnd-agrx-cst;mandates"/>
      <rdfs:domain rdf:resource="&fibo-loan-loan-bt;LoanContract"/>
      <rdfs:range rdf:resource="&fibo-loan-loan-bt;LoanPrincipalRepaymentCommitment"/>
   </owl:ObjectProperty>

   <owl:ObjectProperty rdf:about="&fibo-loan-loan-bt;hasConditions">
      <rdfs:label>has conditions</rdfs:label>
      <rdfs:subPropertyOf rdf:resource="&fibo-fnd-acc-dbt;terms"/>
      <rdfs:domain rdf:resource="&fibo-loan-loan-bt;LoanContract"/>
      <rdfs:range rdf:resource="&fibo-loan-loan-bt;LoanConditions"/>
   </owl:ObjectProperty>

   <owl:ObjectProperty rdf:about="&fibo-loan-loan-bt;hasPaymentSchedule">
      <rdfs:label>has payment schedule</rdfs:label>
      <rdfs:domain rdf:resource="&fibo-loan-loan-bt;LoanContract"/>
      <rdfs:range rdf:resource="&fibo-loan-loan-bt;LoanPaymentSchedule"/>
   </owl:ObjectProperty>

   <owl:ObjectProperty rdf:about="&fibo-loan-loan-bt;hasProvisions">
      <rdfs:label>has provisions</rdfs:label>
      <rdfs:subPropertyOf rdf:resource="&fibo-fnd-agrx-ext;hasProvisions"/>
      <rdfs:domain rdf:resource="&fibo-loan-loan-bt;LoanContract"/>
      <rdfs:range rdf:resource="&fibo-loan-loan-bt;LoanTerminationProvisions"/>
   </owl:ObjectProperty>

   <owl:ObjectProperty rdf:about="&fibo-loan-loan-bt;hasInterestTerms">
      <rdfs:label>has interest terms</rdfs:label>
      <rdfs:subPropertyOf rdf:resource="&fibo-fnd-acc-dbt;terms"/>
      <rdfs:domain rdf:resource="&fibo-loan-loan-bt;LoanContract"/>
      <rdfs:range rdf:resource="&fibo-loan-loan-bt;LoanInterestPaymentTermsSet"/>
   </owl:ObjectProperty>

   <owl:ObjectProperty rdf:about="&fibo-loan-loan-bt;hasPrincipalTerms">
      <rdfs:label>has principal terms</rdfs:label>
      <rdfs:subPropertyOf rdf:resource="&fibo-fnd-acc-dbt;terms"/>
      <rdfs:domain rdf:resource="&fibo-loan-loan-bt;LoanContract"/>
      <rdfs:range rdf:resource="&fibo-loan-loan-bt;LoanPrincipalRepaymentTermsSet"/>
   </owl:ObjectProperty>

   <owl:ObjectProperty rdf:about="&fibo-loan-loan-bt;mayHave">
      <rdfs:label>may have</rdfs:label>
      <rdfs:subPropertyOf rdf:resource="&fibo-fnd-info-info;details"/>
      <rdfs:domain rdf:resource="&fibo-loan-loan-bt;LoanContract"/>
      <rdfs:range rdf:resource="&fibo-loan-loan-bt;LoanStandardizationDocumentation"/>
   </owl:ObjectProperty>

   <owl:ObjectProperty rdf:about="&fibo-loan-loan-bt;setsOutTermsFor">
      <rdfs:label>sets out terms for</rdfs:label>
      <skos:definition>Extended credit (debt or Credit depending on the Viewpoint) has terms set out in a Contract, governing the terms fo extension of the cerdit, payment of interest, principal repayment and any other required clauses defining conditions of the loan or credit. Note feb 2010: term created in Sept 2008 as part of upper ontology. Review and perhaps specialise the kind of contract this relationship comes from.</skos:definition>
      <rdfs:domain rdf:resource="&fibo-loan-loan-bt;LoanContract"/>
      <rdfs:range rdf:resource="&fibo-loan-loan-bt;Loan"/>
   </owl:ObjectProperty>

   <owl:ObjectProperty rdf:about="&fibo-loan-loan-bt;specifies">
      <rdfs:label>specifies</rdfs:label>
      <rdfs:domain rdf:resource="&fibo-loan-loan-bt;LoanContract"/>
      <rdfs:range rdf:resource="&fibo-loan-loan-bt;LoanRetainedAmount"/>
   </owl:ObjectProperty>

   <owl:ObjectProperty rdf:about="&fibo-loan-loan-bt;earlyPrepaymentPenalty">
      <rdfs:label>early prepayment penalty</rdfs:label>
      <skos:definition>The amount to be paid as a penalty in the event of early payment of the loan.</skos:definition>
      <rdfs:domain rdf:resource="&fibo-loan-loan-bt;LoanEarlyPrepaymentTermsSet"/>
      <rdfs:range rdf:resource="&fibo-fnd-acc-cur;MoneyAmount"/>
   </owl:ObjectProperty>

   <owl:ObjectProperty rdf:about="&fibo-loan-loan-bt;prepaymentPenaltyPeriod">
      <rdfs:label>prepayment penalty period</rdfs:label>
      <skos:definition>Period during which penalities are incurred for partial or full principal repayment prior to loan maturity. MISMO definition: "Information specific to calculation of penalities for partial or full principal repayment prior to loan maturity. " There is a penalty for this as well, perhaps as a monetary amount.</skos:definition>
      <rdfs:domain rdf:resource="&fibo-loan-loan-bt;LoanEarlyPrepaymentTermsSet"/>
      <rdfs:range rdf:resource="&fibo-fnd-tim-tim;Duration"/>
   </owl:ObjectProperty>

   <owl:ObjectProperty rdf:about="&fibo-loan-loan-bt;hasBaseRate">
      <rdfs:label>has base rate</rdfs:label>
      <rdfs:domain rdf:resource="&fibo-loan-loan-bt;LoanFloatingInterestPaymentTermsSet"/>
      <rdfs:range rdf:resource="&fibo-ind-ir-ir;InterestReferenceRate"/>
   </owl:ObjectProperty>

   <owl:ObjectProperty rdf:about="&fibo-loan-loan-bt;defines">
      <rdfs:label>defines</rdfs:label>
      <rdfs:subPropertyOf rdf:resource="&fibo-fnd-info-ids;defines"/>
      <rdfs:domain rdf:resource="&fibo-loan-loan-bt;LoanIdentificationScheme"/>
      <rdfs:range rdf:resource="&fibo-loan-loan-bt;LoanIdentifier"/>
   </owl:ObjectProperty>

   <owl:ObjectProperty rdf:about="&fibo-loan-loan-bt;definedIn">
      <rdfs:label>defined in</rdfs:label>
      <rdfs:subPropertyOf rdf:resource="&fibo-fnd-info-ids;definedIn"/>
      <rdfs:domain rdf:resource="&fibo-loan-loan-bt;LoanIdentifier"/>
      <rdfs:range rdf:resource="&fibo-loan-loan-bt;LoanIdentificationScheme"/>
   </owl:ObjectProperty>

   <owl:ObjectProperty rdf:about="&fibo-loan-loan-bt;governedBy">
      <rdfs:label>governed by</rdfs:label>
      <rdfs:domain rdf:resource="&fibo-loan-loan-bt;LoanInterestPaymentCommitment"/>
      <rdfs:range rdf:resource="&fibo-loan-loan-bt;LoanInterestPaymentTermsSet"/>
   </owl:ObjectProperty>

   <owl:ObjectProperty rdf:about="&fibo-loan-loan-bt;loanInterestResetInterval">
      <rdfs:label>loan interest reset interval</rdfs:label>
      <skos:definition>Interest Rate Reset interval - The interval in months at which the interest rate is adjusted (for floating loans)</skos:definition>
      <rdfs:domain rdf:resource="&fibo-loan-loan-bt;LoanInterestPaymentTermsSet"/>
      <rdfs:range rdf:resource="&fibo-fnd-tim-tim;Duration"/>
   </owl:ObjectProperty>

   <owl:ObjectProperty rdf:about="&fibo-loan-loan-bt;hasBaseRate.1">
      <rdfs:label>has base rate</rdfs:label>
      <rdfs:domain rdf:resource="&fibo-loan-loan-bt;LoanInterestPaymentTermsSet"/>
      <rdfs:range rdf:resource="&fibo-ind-ind-ind;MarketBaseRate"/>
   </owl:ObjectProperty>

   <owl:ObjectProperty rdf:about="&fibo-loan-loan-bt;mayBecome">
      <rdfs:label>may become</rdfs:label>
      <rdfs:domain rdf:resource="&fibo-loan-loan-bt;LoanOriginator"/>
      <rdfs:range rdf:resource="&fibo-loan-loan-par;LoanLender"/>
   </owl:ObjectProperty>

   <owl:ObjectProperty rdf:about="&fibo-loan-loan-bt;gracePeriod">
      <rdfs:label>grace period</rdfs:label>
      <skos:definition>The period of time after any due date that the borrower has to fulfil its obligations before a a default (failure to pay) is deemed to have occurred.</skos:definition>
      <rdfs:domain rdf:resource="&fibo-loan-loan-bt;LoanTerminationProvisions"/>
      <rdfs:range rdf:resource="&fibo-fnd-tim-tim;DatePeriod"/>
   </owl:ObjectProperty>

   <owl:ObjectProperty rdf:about="&fibo-loan-loan-bt;hasPrepaymentTerms">
      <rdfs:label>has prepayment terms</rdfs:label>
      <rdfs:subPropertyOf rdf:resource="&fibo-fnd-acc-dbt;terms"/>
      <rdfs:domain rdf:resource="&fibo-loan-loan-bt;LoanContract"/>
      <rdfs:range rdf:resource="&fibo-loan-loan-bt;LoanPrepaymentTermsSet"/>
   </owl:ObjectProperty>

   <owl:ObjectProperty rdf:about="&fibo-loan-loan-bt;preArrangedPaymentFee">
      <rdfs:label>pre arranged payment fee</rdfs:label>
      <skos:definition>The Handling Fee that would be payable in the event of the borrower wishing to make funds available early for application on the schedule due dates (so they are not principal prepayments).</skos:definition>
      <rdfs:domain rdf:resource="&fibo-loan-loan-bt;PaymentArrangementTerms"/>
      <rdfs:range rdf:resource="&fibo-fnd-acc-cur;MoneyAmount"/>
   </owl:ObjectProperty>

   <owl:ObjectProperty rdf:about="&fibo-loan-loan-bt;governedBy.1">
      <rdfs:label>governed by</rdfs:label>
      <rdfs:domain rdf:resource="&fibo-loan-loan-bt;LoanPrincipalRepaymentCommitment"/>
      <rdfs:range rdf:resource="&fibo-loan-loan-bt;LoanPrincipalRepaymentTermsSet"/>
   </owl:ObjectProperty>


  <!--
    ///////////////////////////////////////////////////////////////////////////////////////
    //
    // Data Properties
    //
    ///////////////////////////////////////////////////////////////////////////////////////
    -->


<owl:DatatypeProperty rdf:about="&fibo-loan-loan-bt;buydownExists">
      <rdfs:label>buydown exists</rdfs:label>
      <skos:definition>Whether a third party (usually a builder) is making payments to subsize a borrower.</skos:definition>
      <rdfs:range rdf:resource="&fibo-fnd-utl-bt;yesOrNo"/>
   </owl:DatatypeProperty>

   <owl:DatatypeProperty rdf:about="&fibo-loan-loan-bt;drawDownDate">
      <rdfs:label>draw down date</rdfs:label>
      <skos:definition>The date on which the funds are drawn down, that define the start of the loan.</skos:definition>
      <rdfs:range rdf:resource="http://www.w3.org/2001/XMLSchema#date"/>
   </owl:DatatypeProperty>

   <owl:DatatypeProperty rdf:about="&fibo-loan-loan-bt;loanGuaranteeInsuredPoint">
      <rdfs:label>loan guarantee insured point</rdfs:label>
      <skos:definition>Loan to Value percentage above which losses are insured.</skos:definition>
      <rdfs:range rdf:resource="&fibo-fnd-utl-bt;percentage"/>
   </owl:DatatypeProperty>

   <owl:DatatypeProperty rdf:about="&fibo-loan-loan-bt;loanGuarantorType">
      <rdfs:label>loan guarantor type</rdfs:label>
      <skos:definition>The type of guarantee provider, if applicable. Actiojn: Move down th eGuaranteed Loan.</skos:definition>
      <rdfs:range rdf:resource="http://www.w3.org/2001/XMLSchema#string"/>
   </owl:DatatypeProperty>

   <owl:DatatypeProperty rdf:about="&fibo-loan-loan-bt;loanOriginalAdvanceDate">
      <rdfs:label>loan original advance date</rdfs:label>
      <skos:definition>Loan origination date, that is the date of original loan advance.</skos:definition>
      <rdfs:range rdf:resource="http://www.w3.org/2001/XMLSchema#date"/>
   </owl:DatatypeProperty>

   <owl:DatatypeProperty rdf:about="&fibo-loan-loan-bt;loanOriginationChannelType">
      <rdfs:label>loan origination channel type</rdfs:label>
      <skos:definition>The type of bank, division or organization which was responsible for arranging the loan.</skos:definition>
      <rdfs:range rdf:resource="http://www.w3.org/2001/XMLSchema#string"/>
   </owl:DatatypeProperty>

   <owl:DatatypeProperty rdf:about="&fibo-loan-loan-bt;loanPhase">
      <rdfs:label>loan phase</rdfs:label>
      <rdfs:range rdf:resource="&fibo-loan-tmp-ph;LoanPhaseSelection"/>
   </owl:DatatypeProperty>

   <owl:DatatypeProperty rdf:about="&fibo-loan-loan-bt;loanPurpose">
      <rdfs:label>loan purpose</rdfs:label>
      <skos:definition>The purpose for which the loan has been advanced.</skos:definition>
      <rdfs:range rdf:resource="http://www.w3.org/2001/XMLSchema#string"/>
   </owl:DatatypeProperty>

   <owl:DatatypeProperty rdf:about="&fibo-loan-loan-bt;loanType">
      <rdfs:label>loan type</rdfs:label>
      <skos:definition>The type of loan or purpose for which the loan is extended.</skos:definition>
      <rdfs:range rdf:resource="&fibo-loan-loan-bt;LoanTypeSelection"/>
   </owl:DatatypeProperty>

   <owl:DatatypeProperty rdf:about="&fibo-loan-loan-bt;recourseLoan">
      <rdfs:label>recourse loan</rdfs:label>
      <skos:definition>The only way you get the money back in the event of default is the security. Recourse is where you still have the opportunity to go back to the borrower for the rest of the money.</skos:definition>
      <rdfs:range rdf:resource="&fibo-fnd-utl-bt;yesOrNo"/>
   </owl:DatatypeProperty>

   <owl:DatatypeProperty rdf:about="&fibo-loan-loan-bt;secured">
      <rdfs:label>secured</rdfs:label>
      <skos:definition>Whether the loan is secured. Further Details: All loans are either secured or unsecured All secured loans are secured by some asset or some guaranty Guaranties have various forms. Guaranties have a guarantor. The guarantor may or may not elect to introduce some collateral of their own. Guarantor may or may not be Co-borrower.</skos:definition>
      <rdfs:range rdf:resource="&fibo-fnd-utl-bt;yesOrNo"/>
   </owl:DatatypeProperty>

   <owl:DatatypeProperty rdf:about="&fibo-loan-loan-bt;subsidyPeriodEndDate">
      <rdfs:label>subsidy period end date</rdfs:label>
      <skos:definition>Subsidy Period - date at which subsidy period ends</skos:definition>
      <rdfs:range rdf:resource="http://www.w3.org/2001/XMLSchema#date"/>
   </owl:DatatypeProperty>

   <owl:DatatypeProperty rdf:about="&fibo-loan-loan-bt;aRMConvertible">
      <rdfs:label>a r m convertible</rdfs:label>
      <skos:definition>Whether the Loan can be converted into an ARM.</skos:definition>
      <rdfs:range rdf:resource="&fibo-fnd-utl-bt;yesOrNo"/>
   </owl:DatatypeProperty>

   <owl:DatatypeProperty rdf:about="&fibo-loan-loan-bt;assumable">
      <rdfs:label>assumable</rdfs:label>
      <skos:definition>Whethre another borrower may take ownership of the property and assume the payments on this loan.</skos:definition>
      <rdfs:range rdf:resource="&fibo-fnd-utl-bt;yesOrNo"/>
   </owl:DatatypeProperty>

   <owl:DatatypeProperty rdf:about="&fibo-loan-loan-bt;escrowApplicable">
      <rdfs:label>escrow applicable</rdfs:label>
      <skos:definition>Whether the servicer is contractually responsible for maintaining an escrow against the account for payment of txes and insurance.</skos:definition>
      <rdfs:range rdf:resource="&fibo-fnd-utl-bt;yesOrNo"/>
   </owl:DatatypeProperty>

   <owl:DatatypeProperty rdf:about="&fibo-loan-loan-bt;loanAmortizationPaymentsNumber">
      <rdfs:label>loan amortization payments number</rdfs:label>
      <skos:definition>The number of payments contractually required at origination to repay the loan. For monthly paying loans this is the number of months from the contractual first payment date to the maturity date.</skos:definition>
      <rdfs:range rdf:resource="&fibo-fnd-utl-bt;number"/>
   </owl:DatatypeProperty>

   <owl:DatatypeProperty rdf:about="&fibo-loan-loan-bt;loanAnnualPrePaymentsRate">
      <rdfs:label>loan annual pre payments rate</rdfs:label>
      <skos:definition>Percentage amount of pre-payments allowed (without penalty ) under the loan contract in any given year</skos:definition>
      <rdfs:range rdf:resource="&fibo-fnd-utl-bt;percentage"/>
   </owl:DatatypeProperty>

   <owl:DatatypeProperty rdf:about="&fibo-loan-loan-bt;loanFurtherAdvancesAllowed">
      <rdfs:label>loan further advances allowed</rdfs:label>
      <skos:definition>Whether the lender allows the borrower the possibility to have further advances i.e. advances above the original loan balance.</skos:definition>
      <rdfs:range rdf:resource="&fibo-fnd-utl-bt;yesOrNo"/>
   </owl:DatatypeProperty>

   <owl:DatatypeProperty rdf:about="&fibo-loan-loan-bt;loanPeriodicPaymentType">
      <rdfs:label>loan periodic payment type</rdfs:label>
      <skos:definition>Periodic payment type. May combine interst and principal amounts. See selection of values. May also be principal interest and ESCROW.</skos:definition>
      <rdfs:range rdf:resource="http://www.w3.org/2001/XMLSchema#string"/>
   </owl:DatatypeProperty>

   <owl:DatatypeProperty rdf:about="&fibo-loan-loan-bt;loanRetainedAmountDate">
      <rdfs:label>loan retained amount date</rdfs:label>
      <skos:definition>Date when the retained amount is to be drawn by.</skos:definition>
      <rdfs:range rdf:resource="http://www.w3.org/2001/XMLSchema#dateTime"/>
   </owl:DatatypeProperty>

   <owl:DatatypeProperty rdf:about="&fibo-loan-loan-bt;maturityDate">
      <rdfs:label>maturity date</rdfs:label>
      <skos:definition>The date when the loan matures and is due to be repaid.</skos:definition>
      <rdfs:range rdf:resource="http://www.w3.org/2001/XMLSchema#dateTime"/>
   </owl:DatatypeProperty>

   <owl:DatatypeProperty rdf:about="&fibo-loan-loan-bt;applicableToSameLenderRefinance">
      <rdfs:label>applicable to same lender refinance</rdfs:label>
      <skos:definition>Whether the penalty is specified as being for the loan being paid off in the event of a refinance with same lender. No = these terms relate to penalties where the loan is not so refinanced.</skos:definition>
      <rdfs:range rdf:resource="&fibo-fnd-utl-bt;yesOrNo"/>
   </owl:DatatypeProperty>

   <owl:DatatypeProperty rdf:about="&fibo-loan-loan-bt;applicableToSameLenderRefinance.1">
      <rdfs:label>applicable to same lender refinance</rdfs:label>
      <skos:definition>Whether the penalty is specified as being for the loan being paid off in the event of a refinance with same lender. Yes = these terms define the penalty payable when the debt is refinanced by arrangement with the same lender.</skos:definition>
      <rdfs:range rdf:resource="&fibo-fnd-utl-bt;yesOrNo"/>
   </owl:DatatypeProperty>

   <owl:DatatypeProperty rdf:about="&fibo-loan-loan-bt;applicableToSameLenderRefinance.2">
      <rdfs:label>applicable to same lender refinance</rdfs:label>
      <skos:definition>Whether the penalty is specified as being for the loan being paid off in the event of a refinance with same lender.</skos:definition>
      <rdfs:range rdf:resource="&fibo-fnd-utl-bt;yesOrNo"/>
   </owl:DatatypeProperty>

   <owl:DatatypeProperty rdf:about="&fibo-loan-loan-bt;prepaymentPenaltyWaiver">
      <rdfs:label>prepayment penalty waiver</rdfs:label>
      <skos:definition>Whether the Loan Contract includes a provision for the lender to waive the prepayment penalty at their discretion.</skos:definition>
      <rdfs:range rdf:resource="&fibo-fnd-utl-bt;yesOrNo"/>
   </owl:DatatypeProperty>

   <owl:DatatypeProperty rdf:about="&fibo-loan-loan-bt;spread">
      <rdfs:label>spread</rdfs:label>
      <skos:definition>The percentage of interest added to the base rate.</skos:definition>
      <rdfs:range rdf:resource="&fibo-fnd-utl-bt;percentage"/>
   </owl:DatatypeProperty>

   <owl:DatatypeProperty rdf:about="&fibo-loan-loan-bt;loanInterestPaymentFrequency">
      <rdfs:label>loan interest payment frequency</rdfs:label>
      <skos:definition>Payment Frequency - Frequency of payments due, i.e. number of months between payments.</skos:definition>
      <rdfs:range rdf:resource="&fibo-fnd-tim-tim;Frequency"/>
   </owl:DatatypeProperty>

   <owl:DatatypeProperty rdf:about="&fibo-loan-loan-bt;loanInterestRateCap">
      <rdfs:label>loan interest rate cap</rdfs:label>
      <skos:definition>The cap on the interest rate chargeable, if there is one.</skos:definition>
      <rdfs:range rdf:resource="&fibo-fnd-utl-bt;percentage"/>
   </owl:DatatypeProperty>

   <owl:DatatypeProperty rdf:about="&fibo-loan-loan-bt;loanInterestRateType">
      <rdfs:label>loan interest rate type</rdfs:label>
      <skos:definition>Loan Interest Rate Type.</skos:definition>
      <rdfs:range rdf:resource="http://www.w3.org/2001/XMLSchema#string"/>
   </owl:DatatypeProperty>

   <owl:DatatypeProperty rdf:about="&fibo-loan-loan-bt;renegotiable">
      <rdfs:label>renegotiable</rdfs:label>
      <skos:definition>Whether the terms for payment of interest can be renegotiated during the life of the loan.</skos:definition>
      <rdfs:range rdf:resource="&fibo-fnd-utl-bt;yesOrNo"/>
   </owl:DatatypeProperty>

   <owl:DatatypeProperty rdf:about="&fibo-loan-loan-bt;penaltyInterestAppliedTo">
      <rdfs:label>penalty interest applied to</rdfs:label>
      <skos:definition>The balance to which the penalty interest is to be applied.</skos:definition>
      <rdfs:range rdf:resource="&fibo-loan-loan-bt;LoanPenaltyInterestApplicationSelection"/>
   </owl:DatatypeProperty>

   <owl:DatatypeProperty rdf:about="&fibo-loan-loan-bt;prepaymentPenaltyInterest">
      <rdfs:label>prepayment penalty interest</rdfs:label>
      <skos:definition>Prepayment Penalty Interest.</skos:definition>
      <rdfs:range rdf:resource="&fibo-fnd-utl-bt;percentage"/>
   </owl:DatatypeProperty>

   <owl:DatatypeProperty rdf:about="&fibo-loan-loan-bt;prepaymentThreshold">
      <rdfs:label>prepayment threshold</rdfs:label>
      <skos:definition>Percentage amount of pre-payments allowed under the product per year. This is for mortgages that allow a certain threshold of pre-payments (ie 10%) before charges are incurred.</skos:definition>
      <rdfs:range rdf:resource="&fibo-fnd-utl-bt;percentage"/>
   </owl:DatatypeProperty>

   <owl:DatatypeProperty rdf:about="&fibo-loan-loan-bt;baloon">
      <rdfs:label>baloon</rdfs:label>
      <skos:definition>Whether the loan will or will not amortize the loan balance fully by the maturity date.</skos:definition>
      <rdfs:range rdf:resource="&fibo-fnd-utl-bt;yesOrNo"/>
   </owl:DatatypeProperty>

   <owl:DatatypeProperty rdf:about="&fibo-loan-loan-bt;retainedUntil">
      <rdfs:label>retained until</rdfs:label>
      <skos:definition>Date when the retained amount is to be drawn by.</skos:definition>
      <rdfs:range rdf:resource="&fibo-fnd-tim-tim;Date"/>
   </owl:DatatypeProperty>

   <owl:DatatypeProperty rdf:about="&fibo-loan-loan-bt;docType">
      <rdfs:label>doc type</rdfs:label>
      <rdfs:range rdf:resource="&fibo-loan-loan-loan;LoanStandarizationDocumentType"/>
   </owl:DatatypeProperty>

   <owl:DatatypeProperty rdf:about="&fibo-loan-loan-bt;riskLevel">
      <rdfs:label>risk level</rdfs:label>
      <rdfs:range rdf:resource="&fibo-loan-loan-loan;LoanDocumentRiskLevel"/>
   </owl:DatatypeProperty>

   <owl:DatatypeProperty rdf:about="&fibo-loan-loan-bt;renegotiable.1">
      <rdfs:label>renegotiable</rdfs:label>
      <rdfs:range rdf:resource="&fibo-fnd-utl-bt;yesOrNo"/>
   </owl:DatatypeProperty>


  <!--
    ///////////////////////////////////////////////////////////////////////////////////////
    //
    // Annotation Properties
    //
    ///////////////////////////////////////////////////////////////////////////////////////
    -->



  <!--
    ///////////////////////////////////////////////////////////////////////////////////////
    //
    // Classes
    //
    ///////////////////////////////////////////////////////////////////////////////////////
    -->


<owl:Class rdf:about="&fibo-loan-loan-bt;Loan">
      <rdfs:label>loan</rdfs:label>
      <skos:definition>An amount of money, drawn down by one party (the borrower) from a credit tranche made available by another party (the lender) at a specific point in time. Formal terms for the loan are defined in a Loan Contract.</skos:definition>
      <rdfs:subClassOf rdf:resource="&fibo-fnd-acc-dbt;DebtFinance"/>
   </owl:Class>

   <owl:Class rdf:about="&fibo-loan-loan-bt;LoanBorrowerCommitment">
      <rdfs:label>loan borrower commitment</rdfs:label>
      <skos:definition>The commitment of a given borrower to be a borrower and to repay this loan.</skos:definition>
      <rdfs:subClassOf rdf:resource="&fibo-fnd-agrx-cst;ContractualCommitment"/>
   </owl:Class>

   <owl:Class rdf:about="&fibo-loan-loan-bt;LoanConditions">
      <rdfs:label>loan conditions</rdfs:label>
      <skos:definition>Conditions which must be met by the Borrower during the course of the loan. Breach of these conditions will have predetermined consequences.</skos:definition>
      <rdfs:subClassOf rdf:resource="&fibo-fnd-acc-dbt;DebtContractTermsSet"/>
   </owl:Class>

   <owl:Class rdf:about="&fibo-loan-loan-bt;LoanContract">
      <rdfs:label>loan contract</rdfs:label>
      <skos:definition>The Contract which embodies a loan from one party (the Lender) to another party (the Borrower).</skos:definition>
      <rdfs:subClassOf rdf:resource="&fibo-fnd-agr-ctr;WrittenContract"/>
      <rdfs:subClassOf rdf:resource="&fibo-fnd-agr-ctr;BilateralContract"/>
   </owl:Class>

   <owl:Class rdf:about="&fibo-loan-loan-bt;LoanEarlyPrepaymentHardPenaltyTermsSet">
      <rdfs:label>loan early prepayment hard penalty terms set</rdfs:label>
      <skos:definition>Early repayment penalty in the event of the loan being paid off without any refinancing with the same lender.</skos:definition>
      <rdfs:subClassOf rdf:resource="&fibo-loan-loan-bt;LoanEarlyPrepaymentTermsSet"/>
   </owl:Class>

   <owl:Class rdf:about="&fibo-loan-loan-bt;LoanEarlyPrepaymentSoftPenaltyTermsSet">
      <rdfs:label>loan early prepayment soft penalty terms set</rdfs:label>
      <skos:definition>Early repayment penalty in the event of the loan being paid off in order to refinance with the same lender.</skos:definition>
   </owl:Class>

   <owl:Class rdf:about="&fibo-loan-loan-bt;LoanEarlyPrepaymentTermsSet">
      <rdfs:label>loan early prepayment terms set</rdfs:label>
      <skos:definition>Terms governing the prepayment in full of a loan early in the life of that loan.</skos:definition>
      <rdfs:subClassOf rdf:resource="&fibo-loan-loan-bt;LoanPrepaymentTermsSet"/>
   </owl:Class>

   <owl:Class rdf:about="&fibo-loan-loan-bt;LoanFixedInterestPaymentTermsSet">
      <rdfs:label>loan fixed interest payment terms set</rdfs:label>
      <rdfs:subClassOf rdf:resource="&fibo-loan-loan-bt;LoanInterestPaymentTermsSet"/>
   </owl:Class>

   <owl:Class rdf:about="&fibo-loan-loan-bt;LoanFloatingInterestPaymentTermsSet">
      <rdfs:label>loan floating interest payment terms set</rdfs:label>
   </owl:Class>

   <owl:Class rdf:about="&fibo-loan-loan-bt;LoanIdentificationScheme">
      <rdfs:label>loan identification scheme</rdfs:label>
      <skos:definition>A scheme for formal identification of loans. Further notes: May be a published, public scheme or an internal scheme. MAy not be a database-specific key.</skos:definition>
      <rdfs:subClassOf rdf:resource="&fibo-fnd-info-ids;IdentificationScheme"/>
   </owl:Class>

   <owl:Class rdf:about="&fibo-loan-loan-bt;LoanIdentifier">
      <rdfs:label>loan identifier</rdfs:label>
      <skos:definition>A formal identification code allocated to loans.</skos:definition>
      <rdfs:subClassOf rdf:resource="&fibo-fnd-info-ids;Identifier"/>
   </owl:Class>

   <owl:Class rdf:about="&fibo-loan-loan-bt;LoanInterestPaymentCommitment">
      <rdfs:label>loan interest payment commitment</rdfs:label>
      <skos:definition>A commitment by the borrower of a loan to pay interest on that loan or on amounts of that loan.</skos:definition>
      <rdfs:subClassOf rdf:resource="&fibo-loan-loan-bt;LoanBorrowerCommitment"/>
   </owl:Class>

   <owl:Class rdf:about="&fibo-loan-loan-bt;LoanInterestPaymentTermsSet">
      <rdfs:label>loan interest payment terms set</rdfs:label>
      <skos:definition>Contractual terms governing the payment of interest on the loan.</skos:definition>
      <rdfs:subClassOf rdf:resource="&fibo-fnd-acc-dbt;DebtInterestPaymentTermsSet"/>
   </owl:Class>

   <owl:Class rdf:about="&fibo-loan-loan-bt;LoanOngoingPrepaymentTermsSet">
      <rdfs:label>loan ongoing prepayment terms set</rdfs:label>
      <skos:definition>Terms governing prepayments of the principal on a loan by the borrower throughout the life of the loan.</skos:definition>
   </owl:Class>

   <owl:Class rdf:about="&fibo-loan-loan-bt;LoanOriginator">
      <rdfs:label>loan originator</rdfs:label>
      <skos:definition>The party which finds the lender for the loan, for the borrower.</skos:definition>
      <rdfs:subClassOf rdf:resource="&fibo-loan-loan-par;LoanThirdParty"/>
   </owl:Class>

   <owl:Class rdf:about="&fibo-loan-loan-bt;LoanParty">
      <rdfs:label>loan party</rdfs:label>
      <skos:definition>A Party to the Loan.</skos:definition>
      <rdfs:subClassOf rdf:resource="&fibo-fnd-pty-pty;PartyInRole"/>
   </owl:Class>

   <owl:Class rdf:about="&fibo-loan-loan-bt;LoanPaymentSchedule">
      <rdfs:label>loan payment schedule</rdfs:label>
      <skos:definition>The schedule for payments made by the borrower.</skos:definition>
   </owl:Class>

   <owl:Class rdf:about="&fibo-loan-loan-bt;LoanPrepaymentTermsSet">
      <rdfs:label>loan prepayment terms set</rdfs:label>
      <skos:definition>Terms governing prepayments of the principal on a loan by the borrower.</skos:definition>
      <rdfs:subClassOf rdf:resource="&fibo-loan-loan-bt;LoanPrincipalRepaymentTermsSet"/>
   </owl:Class>

   <owl:Class rdf:about="&fibo-loan-loan-bt;LoanPrincipalRepaymentCommitment">
      <rdfs:label>loan principal repayment commitment</rdfs:label>
      <skos:definition>A commitment by a borrower to repay the principal on a loan under the terms described.</skos:definition>
   </owl:Class>

   <owl:Class rdf:about="&fibo-loan-loan-bt;LoanPrincipalRepaymentTermsSet">
      <rdfs:label>loan principal repayment terms set</rdfs:label>
      <skos:definition>Terms governing the repayment of principal of the loan.</skos:definition>
      <rdfs:subClassOf rdf:resource="&fibo-fnd-acc-dbt;DebtPrincipalRepaymentTermsSet"/>
   </owl:Class>

   <owl:Class rdf:about="&fibo-loan-loan-bt;LoanRetainedAmount">
      <rdfs:label>loan retained amount</rdfs:label>
      <skos:definition>Retained amount, an amount the Issuer will be obliged to fund to the borrower at a later date, for example construction deposit.</skos:definition>
      <rdfs:subClassOf rdf:resource="&fibo-fnd-acc-cur;MoneyAmount"/>
   </owl:Class>

   <owl:Class rdf:about="&fibo-loan-loan-bt;LoanStandardizationDocumentation">
      <rdfs:label>loan standardization documentation</rdfs:label>
      <skos:definition>Very specific categorization of documentation obtained by the lender at the time of origination to qualify a borrower. Documentation Types vary from lender to lender and need to be completely understood. takes a code list in the data world see eg S&P codes of these. not exhaustive? example tax returns etc. categorize as hi low or medium type of doc risk there are also 'no doc' mtges</skos:definition>
      <rdfs:subClassOf rdf:resource="&fibo-fnd-info-info;WrittenInformation"/>
   </owl:Class>

   <owl:Class rdf:about="&fibo-loan-loan-bt;LoanTerminationProvisions">
      <rdfs:label>loan termination provisions</rdfs:label>
      <rdfs:subClassOf rdf:resource="&fibo-fnd-agrx-ext;TerminationProvisions"/>
   </owl:Class>

   <owl:Class rdf:about="&fibo-loan-loan-bt;LoanVariableInterestPaymentTermsSet">
      <rdfs:label>loan variable interest payment terms set</rdfs:label>
   </owl:Class>

   <owl:Class rdf:about="&fibo-loan-loan-bt;PaymentArrangementTerms">
      <rdfs:label>payment arrangement terms</rdfs:label>
      <skos:definition>Terms covering other arrangements for payments such as paying scheduled payments early to be applied on the scheduled payment dates.</skos:definition>
   </owl:Class>


  <!--
    ///////////////////////////////////////////////////////////////////////////////////////
    //
    // Individuals
    //
    ///////////////////////////////////////////////////////////////////////////////////////
    -->


</rdf:RDF>