<?xml version="1.0" encoding="UTF-8"?>
<!DOCTYPE rdf:RDF [
	<!ENTITY dct "http://purl.org/dc/terms/">
	<!ENTITY fibo-bp-iss-doc "https://spec.edmcouncil.org/fibo/ontology/BP/SecuritiesIssuance/IssuanceDocuments/">
	<!ENTITY fibo-bp-iss-trm "https://spec.edmcouncil.org/fibo/ontology/BP/SecuritiesIssuance/IssuanceProcessTerms/">
	<!ENTITY fibo-fnd-agr-ctr "https://spec.edmcouncil.org/fibo/ontology/FND/Agreements/Contracts/">
	<!ENTITY fibo-fnd-inf-doc "https://spec.edmcouncil.org/fibo/ontology/FND/InformationExt/Documentation/">
	<!ENTITY fibo-fnd-inf-inf "https://spec.edmcouncil.org/fibo/ontology/FND/InformationExt/InfoCore/">
	<!ENTITY fibo-fnd-law-cor "https://spec.edmcouncil.org/fibo/ontology/FND/Law/LegalCore/">
	<!ENTITY fibo-fnd-utl-av "https://spec.edmcouncil.org/fibo/ontology/FND/Utilities/AnnotationVocabulary/">
	<!ENTITY fibo-sec-sec-iss "https://spec.edmcouncil.org/fibo/ontology/SEC/Securities/SecuritiesIssuance/">
	<!ENTITY owl "http://www.w3.org/2002/07/owl#">
	<!ENTITY rdf "http://www.w3.org/1999/02/22-rdf-syntax-ns#">
	<!ENTITY rdfs "http://www.w3.org/2000/01/rdf-schema#">
	<!ENTITY skos "http://www.w3.org/2004/02/skos/core#">
	<!ENTITY xsd "http://www.w3.org/2001/XMLSchema#">
]>
<rdf:RDF xml:base="https://spec.edmcouncil.org/fibo/ontology/BP/SecuritiesIssuance/IssuanceDocuments/"
	xmlns:dct="http://purl.org/dc/terms/"
	xmlns:fibo-bp-iss-doc="https://spec.edmcouncil.org/fibo/ontology/BP/SecuritiesIssuance/IssuanceDocuments/"
	xmlns:fibo-bp-iss-trm="https://spec.edmcouncil.org/fibo/ontology/BP/SecuritiesIssuance/IssuanceProcessTerms/"
	xmlns:fibo-fnd-agr-ctr="https://spec.edmcouncil.org/fibo/ontology/FND/Agreements/Contracts/"
	xmlns:fibo-fnd-inf-doc="https://spec.edmcouncil.org/fibo/ontology/FND/InformationExt/Documentation/"
	xmlns:fibo-fnd-inf-inf="https://spec.edmcouncil.org/fibo/ontology/FND/InformationExt/InfoCore/"
	xmlns:fibo-fnd-law-cor="https://spec.edmcouncil.org/fibo/ontology/FND/Law/LegalCore/"
	xmlns:fibo-fnd-utl-av="https://spec.edmcouncil.org/fibo/ontology/FND/Utilities/AnnotationVocabulary/"
	xmlns:fibo-sec-sec-iss="https://spec.edmcouncil.org/fibo/ontology/SEC/Securities/SecuritiesIssuance/"
	xmlns:owl="http://www.w3.org/2002/07/owl#"
	xmlns:rdf="http://www.w3.org/1999/02/22-rdf-syntax-ns#"
	xmlns:rdfs="http://www.w3.org/2000/01/rdf-schema#"
	xmlns:skos="http://www.w3.org/2004/02/skos/core#"
	xmlns:xsd="http://www.w3.org/2001/XMLSchema#">
	
	<owl:Ontology rdf:about="https://spec.edmcouncil.org/fibo/ontology/BP/SecuritiesIssuance/IssuanceDocuments/">
		<rdfs:label xml:lang="en">IssuanceDocuments</rdfs:label>
		<dct:abstract>Ontology containing concepts about types of documentation that are used, referred to or generated by aspects of securities issuance processes.</dct:abstract>
		<owl:imports rdf:resource="https://spec.edmcouncil.org/fibo/ontology/BP/SecuritiesIssuance/DebtIssuance/"/>
		<owl:imports rdf:resource="https://spec.edmcouncil.org/fibo/ontology/BP/SecuritiesIssuance/IssuanceProcessTerms/"/>
		<owl:imports rdf:resource="https://spec.edmcouncil.org/fibo/ontology/FBC/FinancialInstruments/FinancialInstruments/"/>
		<owl:imports rdf:resource="https://spec.edmcouncil.org/fibo/ontology/FND/Agreements/Contracts/"/>
		<owl:imports rdf:resource="https://spec.edmcouncil.org/fibo/ontology/FND/InformationExt/Documentation/"/>
		<owl:imports rdf:resource="https://spec.edmcouncil.org/fibo/ontology/FND/InformationExt/InfoCore/"/>
		<owl:imports rdf:resource="https://spec.edmcouncil.org/fibo/ontology/FND/Law/LegalCore/"/>
		<owl:imports rdf:resource="https://spec.edmcouncil.org/fibo/ontology/FND/Relations/Relations/"/>
		<owl:imports rdf:resource="https://spec.edmcouncil.org/fibo/ontology/FND/Utilities/AnnotationVocabulary/"/>
		<owl:imports rdf:resource="https://spec.edmcouncil.org/fibo/ontology/SEC/Securities/SecuritiesIssuance/"/>
		<owl:versionIRI rdf:resource="https://spec.edmcouncil.org/fibo/ontology/BP/SecuritiesIssuance/IssuanceDocuments/"/>
		<fibo-fnd-utl-av:hasMaturityLevel rdf:resource="&fibo-fnd-utl-av;Provisional"/>
	</owl:Ontology>
	
	<owl:Class rdf:about="&fibo-bp-iss-doc;Indenture">
		<rdfs:subClassOf rdf:resource="&fibo-bp-iss-doc;SecuritiesIssuanceAgreement"/>
		<rdfs:subClassOf rdf:resource="&fibo-fnd-agr-ctr;WrittenContract"/>
		<rdfs:label xml:lang="en">indenture</rdfs:label>
		<skos:definition xml:lang="en">A written contract, also known as a &quot;Deed of Trust&quot;, under which bonds and debentures are issued, setting forth maturity date, interest rate, redemption rights, call privileges and other terms. Under the rules of the Trust Indenture Act of 1939, the contract is executed by the issuer and a trustee who acts on behalf of the bondholders.</skos:definition>
	</owl:Class>
	
	<owl:Class rdf:about="&fibo-bp-iss-doc;IssuanceTrustAgreement">
		<rdfs:subClassOf rdf:resource="&fibo-bp-iss-doc;SecuritiesIssuanceAgreement"/>
		<rdfs:subClassOf rdf:resource="&fibo-fnd-agr-ctr;WrittenContract"/>
		<rdfs:label xml:lang="en">issuance trust agreement</rdfs:label>
	</owl:Class>
	
	<owl:Class rdf:about="&fibo-bp-iss-doc;OfferingDocumentTerms">
		<rdfs:label xml:lang="en">offering document terms</rdfs:label>
		<skos:definition xml:lang="en">Terms which are contained in the identified Offering Document and are considered legally binding within the Issuance and Offering process, if they exist.</skos:definition>
	</owl:Class>
	
	<owl:Class rdf:about="&fibo-bp-iss-doc;OfferingMemorandum">
		<rdfs:subClassOf rdf:resource="&fibo-bp-iss-doc;SecuritiesIssueMemorandum"/>
		<rdfs:label xml:lang="en">offering memorandum</rdfs:label>
	</owl:Class>
	
	<owl:Class rdf:about="&fibo-bp-iss-doc;PlacementAgreement">
		<rdfs:subClassOf rdf:resource="&fibo-bp-iss-doc;SecuritiesIssuanceAgreement"/>
		<rdfs:subClassOf rdf:resource="&fibo-fnd-agr-ctr;WrittenContract"/>
		<rdfs:label xml:lang="en">placement agreement</rdfs:label>
	</owl:Class>
	
	<owl:Class rdf:about="&fibo-bp-iss-doc;ProspectusTermsSet">
		<rdfs:subClassOf rdf:resource="&fibo-bp-iss-doc;ProvisionalTermsDescription"/>
		<rdfs:subClassOf>
			<owl:Restriction>
				<owl:onProperty rdf:resource="&fibo-bp-iss-doc;becomesOnIssue"/>
				<owl:someValuesFrom rdf:resource="&fibo-sec-sec-iss;SecuritiesContractTerms"/>
			</owl:Restriction>
		</rdfs:subClassOf>
		<rdfs:label xml:lang="en">prospectus terms set</rdfs:label>
		<skos:definition xml:lang="en">A set of terms in a Prospectus which on issue will become the binding Contractual Terms of the Security. For example, Call Terms, Interest Payment Terms.</skos:definition>
		<skos:editorialNote xml:lang="en">becomes: The terms in the Prospectus become legally binding contractual terms of the Security, at issue. (former property, now a restriction)</skos:editorialNote>
	</owl:Class>
	
	<owl:Class rdf:about="&fibo-bp-iss-doc;ProvisionalTermsDescription">
		<rdfs:subClassOf rdf:resource="&fibo-fnd-inf-inf;WrittenInformation"/>
		<rdfs:label xml:lang="en">provisional terms description</rdfs:label>
	</owl:Class>
	
	<owl:Class rdf:about="&fibo-bp-iss-doc;SecuritiesIssuanceAgreement">
		<rdfs:subClassOf rdf:resource="&fibo-fnd-agr-ctr;WrittenContract"/>
		<rdfs:label xml:lang="en">securities issuance agreement</rdfs:label>
		<skos:definition xml:lang="en">A formal agreement, deed or contract in respect of some intended securities issuance.</skos:definition>
	</owl:Class>
	
	<owl:Class rdf:about="&fibo-bp-iss-doc;SecuritiesIssuanceCommunication">
		<rdfs:subClassOf rdf:resource="&fibo-fnd-inf-doc;WrittenCommunication"/>
		<rdfs:label xml:lang="en">securities issuance communication</rdfs:label>
		<skos:definition xml:lang="en">A formal memorandum in respect of some securities issuance.</skos:definition>
		<skos:definition xml:lang="en">A notice, statement, declaration, memorandum or other formal written communication in respect of some securities issue, sent out by or on behalf of the issuers of some intended securities issue.</skos:definition>
	</owl:Class>
	
	<owl:Class rdf:about="&fibo-bp-iss-doc;SecuritiesIssuanceNoticeOfSale">
		<rdfs:subClassOf rdf:resource="&fibo-bp-iss-doc;SecuritiesIssuanceCommunication"/>
		<rdfs:subClassOf rdf:resource="&fibo-fnd-inf-doc;Notice"/>
		<rdfs:label xml:lang="en">securities issuance notice of sale</rdfs:label>
	</owl:Class>
	
	<owl:Class rdf:about="&fibo-bp-iss-doc;SecuritiesIssuanceOfficialStatement">
		<rdfs:subClassOf rdf:resource="&fibo-bp-iss-doc;SecuritiesIssuanceCommunication"/>
		<rdfs:subClassOf rdf:resource="&fibo-fnd-inf-doc;FormalStatement"/>
		<rdfs:label xml:lang="en">securities issuance official statement</rdfs:label>
	</owl:Class>
	
	<owl:Class rdf:about="&fibo-bp-iss-doc;SecuritiesIssueMemorandum">
		<rdfs:subClassOf rdf:resource="&fibo-bp-iss-doc;SecuritiesIssuanceCommunication"/>
		<rdfs:subClassOf rdf:resource="&fibo-fnd-inf-doc;Memorandum"/>
		<rdfs:label xml:lang="en">securities issue memorandum</rdfs:label>
		<skos:definition xml:lang="en">A formal memorandum in respect of some securities issuance.</skos:definition>
	</owl:Class>
	
	<owl:Class rdf:about="&fibo-bp-iss-doc;SecurityDraftProspectus">
		<rdfs:subClassOf rdf:resource="&fibo-fnd-inf-doc;DraftContract"/>
		<rdfs:subClassOf>
			<owl:Restriction>
				<owl:onProperty rdf:resource="&fibo-bp-iss-doc;becomesFinal"/>
				<owl:someValuesFrom rdf:resource="&fibo-bp-iss-doc;SecurityFinalProspectus"/>
			</owl:Restriction>
		</rdfs:subClassOf>
		<rdfs:subClassOf>
			<owl:Restriction>
				<owl:onProperty rdf:resource="&fibo-bp-iss-doc;hasDraftTerms"/>
				<owl:someValuesFrom rdf:resource="&fibo-bp-iss-doc;ProspectusTermsSet"/>
			</owl:Restriction>
		</rdfs:subClassOf>
		<rdfs:subClassOf>
			<owl:Restriction>
				<owl:onProperty rdf:resource="&fibo-fnd-inf-doc;comesIntoEffectAs"/>
				<owl:someValuesFrom rdf:resource="https://spec.edmcouncil.org/fibo/ontology/FBC/FinancialInstruments/FinancialInstruments/Security"/>
			</owl:Restriction>
		</rdfs:subClassOf>
		<rdfs:label xml:lang="en">security draft prospectus</rdfs:label>
		<skos:definition xml:lang="en">The draft prospectus for the issue, as determined prior to marketing the issue. Certain terms in the draft prospectus will be finalized later in the issuance process to become the actual Prospectus. Term origin:DTCC issuance Reviews</skos:definition>
	</owl:Class>
	
	<owl:Class rdf:about="&fibo-bp-iss-doc;SecurityFinalProspectus">
		<rdfs:subClassOf rdf:resource="&fibo-sec-sec-iss;Prospectus"/>
		<rdfs:subClassOf>
			<owl:Restriction>
				<owl:onProperty rdf:resource="&fibo-fnd-agr-ctr;hasContractualElement"/>
				<owl:someValuesFrom rdf:resource="&fibo-bp-iss-doc;ProspectusTermsSet"/>
			</owl:Restriction>
		</rdfs:subClassOf>
		<rdfs:label xml:lang="en">security final prospectus</rdfs:label>
		<skos:definition xml:lang="en">The final Prospectus for an issue describes the Offer Issue, including facts about the issue itself such as closing dates, and known facts about the securities that will form part of that issue.</skos:definition>
		<fibo-fnd-utl-av:explanatoryNote xml:lang="en">Anticipated facts might include expected issue price, yields, pool parameters as appropriate for the type of instrument being issued. Term origin:SMER</fibo-fnd-utl-av:explanatoryNote>
	</owl:Class>
	
	<owl:Class rdf:about="&fibo-bp-iss-doc;SecurityIssuanceCertificate">
		<rdfs:subClassOf rdf:resource="&fibo-fnd-inf-doc;Certificate"/>
		<rdfs:label xml:lang="en">security issuance certificate</rdfs:label>
		<skos:definition xml:lang="en">A formal agreement, deed or contract in respect of some intended securities issuance.</skos:definition>
		<skos:definition xml:lang="en">A formal memorandum in respect of some securities issuance.</skos:definition>
		<skos:definition xml:lang="en">A notice, statement, declaration, memorandum or other formal written communication in respect of some securities issue, sent out by or on behalf of the issuers of some intended securities issue.</skos:definition>
		<skos:definition xml:lang="en">Certificate as defined in DTCC terms for type of Offering Document. REVIEW: It is not known whether this is the security certificate itself, or a certificate relating to the Offering of a new Security or issue.</skos:definition>
	</owl:Class>
	
	<owl:Class rdf:about="&fibo-bp-iss-doc;SecurityIssueOrdinance">
		<rdfs:subClassOf rdf:resource="&fibo-fnd-law-cor;Ordinance"/>
		<rdfs:label xml:lang="en">security issue ordinance</rdfs:label>
	</owl:Class>
	
	<owl:Class rdf:about="&fibo-bp-iss-doc;SecurityTermSheet">
		<rdfs:subClassOf rdf:resource="&fibo-fnd-inf-doc;TermsSheet"/>
		<rdfs:subClassOf>
			<owl:Restriction>
				<owl:onProperty rdf:resource="&fibo-bp-iss-doc;hasProvisionalTerms"/>
				<owl:someValuesFrom rdf:resource="&fibo-bp-iss-doc;TermsSheetTermsSet"/>
			</owl:Restriction>
		</rdfs:subClassOf>
		<rdfs:label xml:lang="en">security term sheet</rdfs:label>
		<skos:definition xml:lang="en">A set of written terms for a future financial security setting out legal or contractual rights, obligations and the like, but not (or not yet) forming part of a set of Contractual Terms of the security contract.</skos:definition>
		<fibo-fnd-utl-av:explanatoryNote xml:lang="en">A typical case would be a termsheet in a prospectus, informing potential investors in something, what terms they will expect when the prospectus becomes a formal contract. Note that Termsheet as defined here, being part of the terms of a future contract, refers to the termsheet for the or each individual tranche (i.e. individual contract). In issues with more than one tranche there may well be one document referred to as &quot;the termsheet&quot; but this would legally be several termsheets in the sense used here. Therefore more than one Termsheet may be included in one physical document. Term origin:MBS PoC Reviews</fibo-fnd-utl-av:explanatoryNote>
	</owl:Class>
	
	<owl:Class rdf:about="&fibo-bp-iss-doc;SeriesDeclaration">
		<rdfs:subClassOf rdf:resource="&fibo-bp-iss-doc;SecuritiesIssuanceCommunication"/>
		<rdfs:subClassOf rdf:resource="&fibo-fnd-inf-doc;Declaration"/>
		<rdfs:label xml:lang="en">series declaration</rdfs:label>
	</owl:Class>
	
	<owl:Class rdf:about="&fibo-bp-iss-doc;ShareUnderwriter">
		<rdfs:subClassOf rdf:resource="&fibo-bp-iss-trm;SecurityUnderwriter"/>
		<rdfs:label xml:lang="en">share underwriter</rdfs:label>
		<skos:definition xml:lang="en">The party which agrees to buy any certificates that are not bought by investors Term origin:SR Modeling</skos:definition>
	</owl:Class>
	
	<owl:Class rdf:about="&fibo-bp-iss-doc;TermsSheetTermsSet">
		<rdfs:subClassOf rdf:resource="&fibo-bp-iss-doc;ProvisionalTermsDescription"/>
		<rdfs:subClassOf>
			<owl:Restriction>
				<owl:onProperty rdf:resource="&fibo-bp-iss-doc;becomesOnIssue"/>
				<owl:someValuesFrom rdf:resource="&fibo-sec-sec-iss;SecuritiesContractTerms"/>
			</owl:Restriction>
		</rdfs:subClassOf>
		<rdfs:label xml:lang="en">terms sheet terms set</rdfs:label>
	</owl:Class>
	
	<owl:ObjectProperty rdf:about="&fibo-bp-iss-doc;becomesFinal">
		<rdfs:subPropertyOf rdf:resource="&fibo-fnd-inf-doc;becomesFormalizedAs"/>
		<rdfs:label xml:lang="en">becomes final</rdfs:label>
		<rdfs:domain rdf:resource="&fibo-bp-iss-doc;SecurityDraftProspectus"/>
		<rdfs:range rdf:resource="&fibo-bp-iss-doc;SecurityFinalProspectus"/>
	</owl:ObjectProperty>
	
	<owl:ObjectProperty rdf:about="&fibo-bp-iss-doc;becomesOnIssue">
		<rdfs:label xml:lang="en">becomes on issue</rdfs:label>
		<rdfs:domain rdf:resource="&fibo-bp-iss-doc;ProvisionalTermsDescription"/>
		<rdfs:range rdf:resource="&fibo-sec-sec-iss;SecuritiesContractTerms"/>
		<skos:definition xml:lang="en">An individual set of terms in a Terms Sheet may become a corresponding set of Terms in an Security. This would happen as part of the Issuance process.</skos:definition>
	</owl:ObjectProperty>
	
	<owl:ObjectProperty rdf:about="&fibo-bp-iss-doc;containsTerms">
		<rdfs:label xml:lang="en">contains terms</rdfs:label>
		<rdfs:domain rdf:resource="&fibo-sec-sec-iss;OfferingDocument"/>
		<rdfs:range rdf:resource="&fibo-bp-iss-doc;OfferingDocumentTerms"/>
	</owl:ObjectProperty>
	
	<owl:ObjectProperty rdf:about="&fibo-bp-iss-doc;definesTerms">
		<rdfs:subPropertyOf rdf:resource="&fibo-fnd-inf-inf;isAbout"/>
		<rdfs:label xml:lang="en">defines terms</rdfs:label>
		<rdfs:domain rdf:resource="&fibo-bp-iss-doc;SecurityTermSheet"/>
		<rdfs:range rdf:resource="&fibo-sec-sec-iss;SecuritiesContractTerms"/>
	</owl:ObjectProperty>
	
	<owl:DatatypeProperty rdf:about="&fibo-bp-iss-doc;documentType">
		<rdfs:label xml:lang="en">document type</rdfs:label>
		<rdfs:domain rdf:resource="&fibo-sec-sec-iss;OfferingDocument"/>
		<rdfs:range rdf:resource="&xsd;string"/>
		<skos:definition xml:lang="en">The type of document that is required to be sent in an Offering to make the securities in the Offering eligible at DTC.</skos:definition>
	</owl:DatatypeProperty>
	
	<owl:ObjectProperty rdf:about="&fibo-bp-iss-doc;hasDraftTerms">
		<rdfs:label xml:lang="en">has draft terms</rdfs:label>
		<rdfs:domain rdf:resource="&fibo-bp-iss-doc;SecurityDraftProspectus"/>
		<rdfs:range rdf:resource="&fibo-bp-iss-doc;ProspectusTermsSet"/>
	</owl:ObjectProperty>
	
	<owl:ObjectProperty rdf:about="&fibo-bp-iss-doc;hasProvisionalTerms">
		<rdfs:label xml:lang="en">has provisional terms</rdfs:label>
		<rdfs:domain rdf:resource="&fibo-bp-iss-doc;SecurityTermSheet"/>
		<rdfs:range rdf:resource="&fibo-bp-iss-doc;TermsSheetTermsSet"/>
	</owl:ObjectProperty>
	
	<owl:DatatypeProperty rdf:about="&fibo-bp-iss-doc;isFinalVersion">
		<rdfs:label xml:lang="en">is final version</rdfs:label>
		<rdfs:domain rdf:resource="&fibo-sec-sec-iss;OfferingDocument"/>
		<rdfs:range rdf:resource="&xsd;boolean"/>
		<skos:definition xml:lang="en">The version of the document, i.e. whether it is a Draft or a Final version. Note: This is not the revision number, if that exists.</skos:definition>
	</owl:DatatypeProperty>
	
	<owl:Class rdf:about="&fibo-sec-sec-iss;OfferingDocument">
		<rdfs:subClassOf>
			<owl:Restriction>
				<owl:onProperty rdf:resource="&fibo-bp-iss-doc;containsTerms"/>
				<owl:someValuesFrom rdf:resource="&fibo-bp-iss-doc;OfferingDocumentTerms"/>
			</owl:Restriction>
		</rdfs:subClassOf>
		<rdfs:subClassOf>
			<owl:Restriction>
				<owl:onProperty rdf:resource="&fibo-fnd-inf-doc;identifiedAs"/>
				<owl:someValuesFrom>
					<owl:Class>
						<owl:unionOf rdf:parseType="Collection">
							<rdf:Description rdf:about="&fibo-bp-iss-doc;SecuritiesIssuanceAgreement">
							</rdf:Description>
							<rdf:Description rdf:about="&fibo-bp-iss-doc;SecuritiesIssuanceCommunication">
							</rdf:Description>
							<rdf:Description rdf:about="&fibo-bp-iss-doc;SecurityDraftProspectus">
							</rdf:Description>
							<rdf:Description rdf:about="&fibo-bp-iss-doc;SecurityFinalProspectus">
							</rdf:Description>
							<rdf:Description rdf:about="&fibo-bp-iss-doc;SecurityIssuanceCertificate">
							</rdf:Description>
							<rdf:Description rdf:about="&fibo-bp-iss-doc;SecurityIssueOrdinance">
							</rdf:Description>
							<rdf:Description rdf:about="&fibo-bp-iss-doc;SecurityTermSheet">
							</rdf:Description>
						</owl:unionOf>
					</owl:Class>
				</owl:someValuesFrom>
			</owl:Restriction>
		</rdfs:subClassOf>
	</owl:Class>

</rdf:RDF>