<?xml version="1.0" encoding="UTF-8"?>
<rdf:RDF xmlns:xsd="http://www.w3.org/2001/XMLSchema#"
         xmlns:sm="http://www.omg.org/techprocess/ab/SpecificationMetadata/"
         xmlns:fibo-fnd-utl-av="http://www.omg.org/spec/EDMC-FIBO/FND/Utilities/AnnotationVocabulary/"
         xmlns:rdf="http://www.w3.org/1999/02/22-rdf-syntax-ns#"
         xmlns:rdfs="http://www.w3.org/2000/01/rdf-schema#"
         xmlns:owl="http://www.w3.org/2002/07/owl#"
         xmlns:skos="http://www.w3.org/2004/02/skos/core#"
         xmlns:dc="http://purl.org/dc/terms/"
         xml:base="http://www.omg.org/spec/EDMC-FIBO/LOAN/Loans/LoansGeneral/">

   <owl:Ontology rdf:about="http://www.omg.org/spec/EDMC-FIBO/LOAN/Loans/LoansGeneral/">
      <owl:imports rdf:resource="http://www.omg.org/spec/EDMC-FIBO/LOAN/Loans/LoanBasicTerms/"/>
   </owl:Ontology>

   <!--Datatypes-->

<rdf:Description rdf:about="http://www.omg.org/spec/EDMC-FIBO/LOAN/Loans/LoansGeneral/IncomeVerificationMethodSelection">
      <skos:definition>Selection of possible methods by which borrower's income was determined.</skos:definition>
      <owl:equivalentClass>
         <rdfs:Datatype>
            <owl:oneOf>
               <rdf:Description>
                  <rdf:first rdf:datatype="http://www.w3.org/2001/XMLSchema#string">Self Certified</rdf:first>
                  <rdf:rest>
                     <rdf:Description>
                        <rdf:first rdf:datatype="http://www.w3.org/2001/XMLSchema#string">Self Certified Confirmation</rdf:first>
                        <rdf:rest>
                           <rdf:Description>
                              <rdf:first rdf:datatype="http://www.w3.org/2001/XMLSchema#string">Verified</rdf:first>
                              <rdf:rest>
                                 <rdf:Description>
                                    <rdf:first rdf:datatype="http://www.w3.org/2001/XMLSchema#string">Non Verified</rdf:first>
                                    <rdf:rest>
                                       <rdf:Description>
                                          <rdf:first rdf:datatype="http://www.w3.org/2001/XMLSchema#string">Other</rdf:first>
                                          <rdf:rest rdf:resource="http://www.w3.org/1999/02/22-rdf-syntax-ns#nil"/>
                                       </rdf:Description>
                                    </rdf:rest>
                                 </rdf:Description>
                              </rdf:rest>
                           </rdf:Description>
                        </rdf:rest>
                     </rdf:Description>
                  </rdf:rest>
               </rdf:Description>
            </owl:oneOf>
         </rdfs:Datatype>
      </owl:equivalentClass>
   </rdf:Description>

   <rdf:Description rdf:about="http://www.omg.org/spec/EDMC-FIBO/LOAN/Loans/LoansGeneral/LoanBorrowerRoleSelection">
      <owl:equivalentClass>
         <rdfs:Datatype>
            <owl:oneOf>
               <rdf:Description>
                  <rdf:first rdf:datatype="http://www.w3.org/2001/XMLSchema#string">Primary</rdf:first>
                  <rdf:rest>
                     <rdf:Description>
                        <rdf:first rdf:datatype="http://www.w3.org/2001/XMLSchema#string">Secondary</rdf:first>
                        <rdf:rest rdf:resource="http://www.w3.org/1999/02/22-rdf-syntax-ns#nil"/>
                     </rdf:Description>
                  </rdf:rest>
               </rdf:Description>
            </owl:oneOf>
         </rdfs:Datatype>
      </owl:equivalentClass>
   </rdf:Description>

   <rdf:Description rdf:about="http://www.omg.org/spec/EDMC-FIBO/LOAN/Loans/LoansGeneral/LoanDocumentRiskLevel">
      <owl:equivalentClass>
         <rdfs:Datatype>
            <owl:oneOf>
               <rdf:Description>
                  <rdf:first rdf:datatype="http://www.w3.org/2001/XMLSchema#string">High</rdf:first>
                  <rdf:rest>
                     <rdf:Description>
                        <rdf:first rdf:datatype="http://www.w3.org/2001/XMLSchema#string">Medium</rdf:first>
                        <rdf:rest>
                           <rdf:Description>
                              <rdf:first rdf:datatype="http://www.w3.org/2001/XMLSchema#string">Low</rdf:first>
                              <rdf:rest rdf:resource="http://www.w3.org/1999/02/22-rdf-syntax-ns#nil"/>
                           </rdf:Description>
                        </rdf:rest>
                     </rdf:Description>
                  </rdf:rest>
               </rdf:Description>
            </owl:oneOf>
         </rdfs:Datatype>
      </owl:equivalentClass>
   </rdf:Description>

   <rdf:Description rdf:about="http://www.omg.org/spec/EDMC-FIBO/LOAN/Loans/LoansGeneral/LoanStandarizationDocumentType">
      <skos:definition>Financial Institution defined categorization of documentation type. This is interpreted from information provided by the seller on both the data file and in their underwriting quidelines. See attached Translation tables. needs work These are (from CDDOCTYPE enumeration in MAT-CODES): Unknown Other Full Full or Alternate Alternative Lite Low - ACTION make sure this isn't Risk Level in other list Limited Reduced Partial Streamline No Documentation No Ratio No Income Verifier No Income Qualifier Stated Documentation ACTION: Make sure these are all mutually exclusive, then implement as selection list entries.</skos:definition>
      <owl:equivalentClass>
         <rdfs:Datatype>
            <owl:oneOf/>
         </rdfs:Datatype>
      </owl:equivalentClass>
   </rdf:Description>

   <!--Object Properties-->

<owl:ObjectProperty rdf:about="http://www.omg.org/spec/EDMC-FIBO/LOAN/Loans/LoansGeneral/defines">
      <rdfs:subPropertyOf rdf:resource="http://www.edmcouncil.org/spec/EDMC-SR/FND/Information/Identifiers/defines"/>
      <rdfs:domain rdf:resource="http://www.omg.org/spec/EDMC-FIBO/LOAN/Loans/LoansGeneral/CountryIdentificationScheme"/>
      <rdfs:range rdf:resource="http://www.omg.org/spec/EDMC-FIBO/LOAN/Loans/LoansGeneral/CountryIdentifier"/>
   </owl:ObjectProperty>

   <owl:ObjectProperty rdf:about="http://www.omg.org/spec/EDMC-FIBO/LOAN/Loans/LoansGeneral/definedIn">
      <rdfs:subPropertyOf rdf:resource="http://www.edmcouncil.org/spec/EDMC-SR/FND/Information/Identifiers/definedIn"/>
      <rdfs:domain rdf:resource="http://www.omg.org/spec/EDMC-FIBO/LOAN/Loans/LoansGeneral/CountryIdentifier"/>
      <rdfs:range rdf:resource="http://www.omg.org/spec/EDMC-FIBO/LOAN/Loans/LoansGeneral/CountryIdentificationScheme"/>
   </owl:ObjectProperty>

   <owl:ObjectProperty rdf:about="http://www.omg.org/spec/EDMC-FIBO/LOAN/Loans/LoansGeneral/domiciled">
      <rdfs:domain rdf:resource="http://www.omg.org/spec/EDMC-FIBO/LOAN/LoansTemporal/LoanBorrowersTemporal/PersonalAssessmentFactsAtApproval"/>
      <rdfs:range rdf:resource="http://www.omg.org/spec/EDMC-SR/FND/Law/Jurisdictions/Jurisdiction"/>
   </owl:ObjectProperty>

   <!--Data Properties-->

<!--Annotation Properties-->

<!--Classes-->

<owl:Class rdf:about="http://www.omg.org/spec/EDMC-FIBO/LOAN/Loans/LoansGeneral/CountryIdentificationScheme">
      <rdfs:label>Country Identification Scheme</rdfs:label>
      <skos:definition>The scheme in which the identification code for a country is identified.</skos:definition>
      <skos:editorialNote>Examples are the ISO 2 letter and 3 letter country codes. The scheme must identify which this one is (the same standard has bot, in separate sections, so there may not be an obvious dereferenceable URI for this). Added for MBS PoC work, where there is a more general "Location" ID. Review whether other kinds of location need to also have unique identification codes, and what forms these may take, for example postal codes.</skos:editorialNote>
      <rdfs:subClassOf rdf:resource="http://www.edmcouncil.org/spec/EDMC-SR/FND/Information/Identifiers/IdentificationScheme"/>
   </owl:Class>

   <owl:Class rdf:about="http://www.omg.org/spec/EDMC-FIBO/LOAN/Loans/LoansGeneral/CountryIdentifier">
      <rdfs:label>Country Identifier</rdfs:label>
      <skos:definition>A code for identifying a country</skos:definition>
      <rdfs:subClassOf rdf:resource="http://www.edmcouncil.org/spec/EDMC-SR/FND/Information/Identifiers/Identifier"/>
   </owl:Class>

   <owl:Class rdf:about="http://www.omg.org/spec/EDMC-FIBO/LOAN/Loans/LoansGeneral/UnsubscribedDebt">
      <rdfs:label>Unsubscribed Debt</rdfs:label>
      <rdfs:subClassOf rdf:resource="http://www.omg.org/spec/EDMC-FIBO/SEC/Debt/DebtFoundations/DebtInstruments/PubliclyIssuedDebt"/>
   </owl:Class>

   <!--Individuals-->

</rdf:RDF>