<?xml version="1.0" encoding="UTF-8"?>
<!DOCTYPE rdf:RDF [
	<!ENTITY dct "http://purl.org/dc/terms/">
	<!ENTITY fibo-fnd-plc-adr "https://spec.edmcouncil.org/fibo/ontology/FND/Places/Addresses/">
	<!ENTITY fibo-fnd-plc-loc "https://spec.edmcouncil.org/fibo/ontology/FND/Places/Locations/">
	<!ENTITY fibo-fnd-plc-uspsa "https://spec.edmcouncil.org/fibo/ontology/FND/Places/NorthAmerica/USPostalServiceAddresses/">
	<!ENTITY fibo-fnd-rel-rel "https://spec.edmcouncil.org/fibo/ontology/FND/Relations/Relations/">
	<!ENTITY fibo-fnd-utl-av "https://spec.edmcouncil.org/fibo/ontology/FND/Utilities/AnnotationVocabulary/">
	<!ENTITY lcc-cr "https://www.omg.org/spec/LCC/Countries/CountryRepresentation/">
	<!ENTITY lcc-lr "https://www.omg.org/spec/LCC/Languages/LanguageRepresentation/">
	<!ENTITY owl "http://www.w3.org/2002/07/owl#">
	<!ENTITY rdf "http://www.w3.org/1999/02/22-rdf-syntax-ns#">
	<!ENTITY rdfs "http://www.w3.org/2000/01/rdf-schema#">
	<!ENTITY skos "http://www.w3.org/2004/02/skos/core#">
	<!ENTITY sm "http://www.omg.org/techprocess/ab/SpecificationMetadata/">
	<!ENTITY xsd "http://www.w3.org/2001/XMLSchema#">
]>
<rdf:RDF xml:base="https://spec.edmcouncil.org/fibo/ontology/FND/Places/NorthAmerica/USPostalServiceAddresses/"
	xmlns:dct="http://purl.org/dc/terms/"
	xmlns:fibo-fnd-plc-adr="https://spec.edmcouncil.org/fibo/ontology/FND/Places/Addresses/"
	xmlns:fibo-fnd-plc-loc="https://spec.edmcouncil.org/fibo/ontology/FND/Places/Locations/"
	xmlns:fibo-fnd-plc-uspsa="https://spec.edmcouncil.org/fibo/ontology/FND/Places/NorthAmerica/USPostalServiceAddresses/"
	xmlns:fibo-fnd-rel-rel="https://spec.edmcouncil.org/fibo/ontology/FND/Relations/Relations/"
	xmlns:fibo-fnd-utl-av="https://spec.edmcouncil.org/fibo/ontology/FND/Utilities/AnnotationVocabulary/"
	xmlns:lcc-cr="https://www.omg.org/spec/LCC/Countries/CountryRepresentation/"
	xmlns:lcc-lr="https://www.omg.org/spec/LCC/Languages/LanguageRepresentation/"
	xmlns:owl="http://www.w3.org/2002/07/owl#"
	xmlns:rdf="http://www.w3.org/1999/02/22-rdf-syntax-ns#"
	xmlns:rdfs="http://www.w3.org/2000/01/rdf-schema#"
	xmlns:skos="http://www.w3.org/2004/02/skos/core#"
	xmlns:sm="http://www.omg.org/techprocess/ab/SpecificationMetadata/"
	xmlns:xsd="http://www.w3.org/2001/XMLSchema#">
	
	<owl:Ontology rdf:about="https://spec.edmcouncil.org/fibo/ontology/FND/Places/NorthAmerica/USPostalServiceAddresses/">
		<rdfs:label>U.S. Postal Service Addresses Ontology</rdfs:label>
		<dct:abstract>This ontology augments the Addresses ontology in FND with concepts that conform to the USPS Pub 28.  The USPS provides automated address verification services that use the concepts defined herein for that purpose, and which many financial services entities use for data quality purposes.</dct:abstract>
		<dct:license rdf:datatype="&xsd;anyURI">http://opensource.org/licenses/MIT</dct:license>
		<sm:contentLanguage rdf:datatype="&xsd;anyURI">http://www.w3.org/standards/techs/owl#w3c_all</sm:contentLanguage>
		<sm:contributor>Thematix Partners LLC</sm:contributor>
		<sm:copyright>Copyright (c) 2019-2020 EDM Council, Inc.</sm:copyright>
		<sm:copyright>Copyright (c) 2019-2020 Object Management Group, Inc.</sm:copyright>
		<sm:dependsOn rdf:datatype="&xsd;anyURI">https://spec.edmcouncil.org/fibo/ontology/FND/Places/Addresses/</sm:dependsOn>
		<sm:dependsOn rdf:datatype="&xsd;anyURI">https://spec.edmcouncil.org/fibo/ontology/FND/Places/Locations/</sm:dependsOn>
		<sm:dependsOn rdf:datatype="&xsd;anyURI">https://spec.edmcouncil.org/fibo/ontology/FND/Relations/Relations/</sm:dependsOn>
		<sm:dependsOn rdf:datatype="&xsd;anyURI">https://spec.edmcouncil.org/fibo/ontology/FND/Utilities/AnnotationVocabulary/</sm:dependsOn>
		<sm:dependsOn rdf:datatype="&xsd;anyURI">https://www.omg.org/spec/LCC/</sm:dependsOn>
		<sm:fileAbbreviation>fibo-fnd-plc-uspsa</sm:fileAbbreviation>
		<sm:filename>USPostalServiceAddresses.rdf</sm:filename>
		<rdfs:seeAlso rdf:resource="https://about.usps.com/who/profile/"/>
		<rdfs:seeAlso rdf:resource="https://pe.usps.com/cpim/ftp/pubs/Pub28/pub28.pdf"/>
		<owl:imports rdf:resource="https://spec.edmcouncil.org/fibo/ontology/FND/Places/Addresses/"/>
		<owl:imports rdf:resource="https://spec.edmcouncil.org/fibo/ontology/FND/Places/Locations/"/>
		<owl:imports rdf:resource="https://spec.edmcouncil.org/fibo/ontology/FND/Relations/Relations/"/>
		<owl:imports rdf:resource="https://spec.edmcouncil.org/fibo/ontology/FND/Utilities/AnnotationVocabulary/"/>
		<owl:imports rdf:resource="https://www.omg.org/spec/LCC/Countries/CountryRepresentation/"/>
		<owl:imports rdf:resource="https://www.omg.org/spec/LCC/Languages/LanguageRepresentation/"/>
		<owl:versionIRI rdf:resource="https://spec.edmcouncil.org/fibo/ontology/FND/20200701/Places/NorthAmerica/USPostalServiceAddresses/"/>
		<skos:changeNote>The https://spec.edmcouncil.org/fibo/ontology/FND/20200301/Places/NorthAmerica/USPostalServiceAddresses.rdf version of this ontology was revised to replace uses of hasTag in Relations with hasTag from LCC, as the more complex union of datatypes in the Relations concept is not needed here, and correct a duplicate label.</skos:changeNote>
		<fibo-fnd-utl-av:hasMaturityLevel rdf:resource="&fibo-fnd-utl-av;Release"/>
	</owl:Ontology>
	
	<owl:NamedIndividual rdf:about="&fibo-fnd-plc-adr;Apartment">
		<rdfs:label xml:lang="es">apartmento</rdfs:label>
		<fibo-fnd-utl-av:preferredDesignation>APT</fibo-fnd-utl-av:preferredDesignation>
	</owl:NamedIndividual>
	
	<owl:NamedIndividual rdf:about="&fibo-fnd-plc-adr;Basement">
		<fibo-fnd-utl-av:preferredDesignation>BSMT</fibo-fnd-utl-av:preferredDesignation>
	</owl:NamedIndividual>
	
	<owl:NamedIndividual rdf:about="&fibo-fnd-plc-adr;Building">
		<fibo-fnd-utl-av:preferredDesignation>BLDG</fibo-fnd-utl-av:preferredDesignation>
	</owl:NamedIndividual>
	
	<owl:NamedIndividual rdf:about="&fibo-fnd-plc-adr;Department">
		<rdfs:label xml:lang="es">departamento</rdfs:label>
		<fibo-fnd-utl-av:preferredDesignation>DEPT</fibo-fnd-utl-av:preferredDesignation>
	</owl:NamedIndividual>
	
	<owl:NamedIndividual rdf:about="&fibo-fnd-plc-adr;Floor">
		<fibo-fnd-utl-av:preferredDesignation>FL</fibo-fnd-utl-av:preferredDesignation>
	</owl:NamedIndividual>
	
	<owl:NamedIndividual rdf:about="&fibo-fnd-plc-adr;Front">
		<fibo-fnd-utl-av:preferredDesignation>FRNT</fibo-fnd-utl-av:preferredDesignation>
	</owl:NamedIndividual>
	
	<owl:Class rdf:about="&fibo-fnd-plc-adr;GeographicDirectionalSymbol">
		<owl:equivalentClass>
			<owl:Class>
				<owl:oneOf rdf:parseType="Collection">
					<rdf:Description rdf:about="&fibo-fnd-plc-uspsa;East">
					</rdf:Description>
					<rdf:Description rdf:about="&fibo-fnd-plc-uspsa;North">
					</rdf:Description>
					<rdf:Description rdf:about="&fibo-fnd-plc-uspsa;Northeast">
					</rdf:Description>
					<rdf:Description rdf:about="&fibo-fnd-plc-uspsa;Northwest">
					</rdf:Description>
					<rdf:Description rdf:about="&fibo-fnd-plc-uspsa;South">
					</rdf:Description>
					<rdf:Description rdf:about="&fibo-fnd-plc-uspsa;Southeast">
					</rdf:Description>
					<rdf:Description rdf:about="&fibo-fnd-plc-uspsa;Southwest">
					</rdf:Description>
					<rdf:Description rdf:about="&fibo-fnd-plc-uspsa;West">
					</rdf:Description>
				</owl:oneOf>
			</owl:Class>
		</owl:equivalentClass>
	</owl:Class>
	
	<owl:NamedIndividual rdf:about="&fibo-fnd-plc-adr;Hangar">
		<fibo-fnd-utl-av:preferredDesignation>HNGR</fibo-fnd-utl-av:preferredDesignation>
	</owl:NamedIndividual>
	
	<owl:NamedIndividual rdf:about="&fibo-fnd-plc-adr;Key">
		<fibo-fnd-utl-av:preferredDesignation>KEY</fibo-fnd-utl-av:preferredDesignation>
	</owl:NamedIndividual>
	
	<owl:NamedIndividual rdf:about="&fibo-fnd-plc-adr;Lobby">
		<fibo-fnd-utl-av:preferredDesignation>LBBY</fibo-fnd-utl-av:preferredDesignation>
	</owl:NamedIndividual>
	
	<owl:NamedIndividual rdf:about="&fibo-fnd-plc-adr;Lot">
		<fibo-fnd-utl-av:preferredDesignation>LOT</fibo-fnd-utl-av:preferredDesignation>
	</owl:NamedIndividual>
	
	<owl:NamedIndividual rdf:about="&fibo-fnd-plc-adr;Lower">
		<fibo-fnd-utl-av:preferredDesignation>LOWR</fibo-fnd-utl-av:preferredDesignation>
	</owl:NamedIndividual>
	
	<owl:NamedIndividual rdf:about="&fibo-fnd-plc-adr;Office">
		<fibo-fnd-utl-av:preferredDesignation>OFC</fibo-fnd-utl-av:preferredDesignation>
	</owl:NamedIndividual>
	
	<owl:NamedIndividual rdf:about="&fibo-fnd-plc-adr;Penthouse">
		<fibo-fnd-utl-av:preferredDesignation>PH</fibo-fnd-utl-av:preferredDesignation>
	</owl:NamedIndividual>
	
	<owl:NamedIndividual rdf:about="&fibo-fnd-plc-adr;Pier">
		<fibo-fnd-utl-av:preferredDesignation>PIER</fibo-fnd-utl-av:preferredDesignation>
	</owl:NamedIndividual>
	
	<owl:NamedIndividual rdf:about="&fibo-fnd-plc-adr;Rear">
		<fibo-fnd-utl-av:preferredDesignation>REAR</fibo-fnd-utl-av:preferredDesignation>
	</owl:NamedIndividual>
	
	<owl:NamedIndividual rdf:about="&fibo-fnd-plc-adr;Room">
		<fibo-fnd-utl-av:preferredDesignation>RM</fibo-fnd-utl-av:preferredDesignation>
	</owl:NamedIndividual>
	
	<owl:NamedIndividual rdf:about="&fibo-fnd-plc-adr;Side">
		<fibo-fnd-utl-av:preferredDesignation>SIDE</fibo-fnd-utl-av:preferredDesignation>
	</owl:NamedIndividual>
	
	<owl:NamedIndividual rdf:about="&fibo-fnd-plc-adr;Slip">
		<fibo-fnd-utl-av:preferredDesignation>SLP</fibo-fnd-utl-av:preferredDesignation>
	</owl:NamedIndividual>
	
	<owl:NamedIndividual rdf:about="&fibo-fnd-plc-adr;Space">
		<fibo-fnd-utl-av:preferredDesignation>SPC</fibo-fnd-utl-av:preferredDesignation>
	</owl:NamedIndividual>
	
	<owl:NamedIndividual rdf:about="&fibo-fnd-plc-adr;Stop">
		<fibo-fnd-utl-av:preferredDesignation>STOP</fibo-fnd-utl-av:preferredDesignation>
	</owl:NamedIndividual>
	
	<owl:NamedIndividual rdf:about="&fibo-fnd-plc-adr;Suite">
		<fibo-fnd-utl-av:preferredDesignation>STE</fibo-fnd-utl-av:preferredDesignation>
	</owl:NamedIndividual>
	
	<owl:NamedIndividual rdf:about="&fibo-fnd-plc-adr;Trailer">
		<fibo-fnd-utl-av:preferredDesignation>TRLR</fibo-fnd-utl-av:preferredDesignation>
	</owl:NamedIndividual>
	
	<owl:NamedIndividual rdf:about="&fibo-fnd-plc-adr;Unit">
		<fibo-fnd-utl-av:preferredDesignation>UNIT</fibo-fnd-utl-av:preferredDesignation>
	</owl:NamedIndividual>
	
	<owl:NamedIndividual rdf:about="&fibo-fnd-plc-adr;Upper">
		<fibo-fnd-utl-av:preferredDesignation>UPPR</fibo-fnd-utl-av:preferredDesignation>
	</owl:NamedIndividual>
	
	<owl:Class rdf:about="&fibo-fnd-plc-uspsa;CompleteAddress">
		<rdfs:subClassOf rdf:resource="&fibo-fnd-plc-uspsa;StandardizedAddress"/>
		<rdfs:label>complete address</rdfs:label>
		<skos:definition>delivery address that has all the address elements necessary to allow an exact match with the current Postal Service ZIP+4 and City State files to obtain the finest level of ZIP+4 and delivery point codes for the delivery address</skos:definition>
		<fibo-fnd-utl-av:explanatoryNote>A complete address may be required on mail at some automation rates.</fibo-fnd-utl-av:explanatoryNote>
	</owl:Class>
	
	<owl:Class rdf:about="&fibo-fnd-plc-uspsa;DeliveryAddressCodeSet">
		<rdfs:subClassOf rdf:resource="&lcc-lr;CodeSet"/>
		<rdfs:subClassOf rdf:resource="&lcc-lr;IdentificationScheme"/>
		<rdfs:subClassOf>
			<owl:Restriction>
				<owl:onProperty rdf:resource="&lcc-lr;hasMember"/>
				<owl:someValuesFrom rdf:resource="&fibo-fnd-plc-uspsa;USPostalServiceAddressIdentifier"/>
			</owl:Restriction>
		</rdfs:subClassOf>
		<rdfs:label>delivery address code set</rdfs:label>
		<rdfs:seeAlso rdf:resource="https://pe.usps.com/cpim/ftp/pubs/Pub28/pub28.pdf"/>
		<skos:definition>system of numeric codes that substitute for specified delivery point details according to the U.S. Postal Service Publication 28</skos:definition>
	</owl:Class>
	
	<owl:Class rdf:about="&fibo-fnd-plc-uspsa;DeliveryPointCode">
		<rdfs:subClassOf rdf:resource="&lcc-lr;CodeElement"/>
		<rdfs:subClassOf>
			<owl:Restriction>
				<owl:onProperty rdf:resource="&lcc-lr;isMemberOf"/>
				<owl:onClass rdf:resource="&fibo-fnd-plc-uspsa;DeliveryPointCodeSet"/>
				<owl:qualifiedCardinality rdf:datatype="&xsd;nonNegativeInteger">1</owl:qualifiedCardinality>
			</owl:Restriction>
		</rdfs:subClassOf>
		<rdfs:subClassOf>
			<owl:Restriction>
				<owl:onProperty rdf:resource="&lcc-lr;hasTag"/>
				<owl:onDataRange rdf:resource="&xsd;string"/>
				<owl:qualifiedCardinality rdf:datatype="&xsd;nonNegativeInteger">1</owl:qualifiedCardinality>
			</owl:Restriction>
		</rdfs:subClassOf>
		<rdfs:label>delivery point code</rdfs:label>
		<rdfs:seeAlso rdf:resource="https://pe.usps.com/cpim/ftp/pubs/Pub28/pub28.pdf"/>
		<skos:definition>specific set of digits between 00 and 99 assigned to a delivery point</skos:definition>
		<fibo-fnd-utl-av:explanatoryNote>When combined with the ZIP + 4 code, the delivery point code provides a unique identifier for every deliverable address served by the USPS.  The delivery point digits are almost never printed on mail in human-readable form; instead they are encoded in the POSTNET delivery point barcode (DPBC) or as part of the newer Intelligent Mail Barcode (IMB).</fibo-fnd-utl-av:explanatoryNote>
	</owl:Class>
	
	<owl:Class rdf:about="&fibo-fnd-plc-uspsa;DeliveryPointCodeSet">
		<rdfs:subClassOf rdf:resource="&lcc-lr;CodeSet"/>
		<rdfs:subClassOf>
			<owl:Restriction>
				<owl:onProperty rdf:resource="&lcc-lr;hasMember"/>
				<owl:someValuesFrom rdf:resource="&fibo-fnd-plc-uspsa;DeliveryPointCode"/>
			</owl:Restriction>
		</rdfs:subClassOf>
		<rdfs:label>delivery point code set</rdfs:label>
		<rdfs:seeAlso rdf:resource="https://pe.usps.com/cpim/ftp/pubs/Pub28/pub28.pdf"/>
		<skos:definition>system of numeric codes that substitute for specified delivery point details according to the U.S. Postal Service Publication 28</skos:definition>
	</owl:Class>
	
	<owl:Class rdf:about="&fibo-fnd-plc-uspsa;DepartmentOfStateAddress">
		<rdfs:subClassOf rdf:resource="&fibo-fnd-plc-adr;PhysicalAddress"/>
		<rdfs:subClassOf>
			<owl:Restriction>
				<owl:onProperty rdf:resource="&fibo-fnd-plc-loc;hasCityName"/>
				<owl:hasValue>DPO</owl:hasValue>
			</owl:Restriction>
		</rdfs:subClassOf>
		<rdfs:subClassOf>
			<owl:Restriction>
				<owl:onProperty rdf:resource="&fibo-fnd-rel-rel;comprises"/>
				<owl:onClass rdf:resource="&fibo-fnd-plc-uspsa;DepartmentOfStateUnitComponent"/>
				<owl:qualifiedCardinality rdf:datatype="&xsd;nonNegativeInteger">1</owl:qualifiedCardinality>
			</owl:Restriction>
		</rdfs:subClassOf>
		<rdfs:subClassOf>
			<owl:Restriction>
				<owl:onProperty rdf:resource="&fibo-fnd-rel-rel;comprises"/>
				<owl:onClass rdf:resource="&fibo-fnd-plc-uspsa;Mailbox"/>
				<owl:qualifiedCardinality rdf:datatype="&xsd;nonNegativeInteger">1</owl:qualifiedCardinality>
			</owl:Restriction>
		</rdfs:subClassOf>
		<rdfs:label>Department of State address</rdfs:label>
		<owl:disjointWith rdf:resource="&fibo-fnd-plc-adr;ConventionalStreetAddress"/>
		<skos:definition>delivery address whose delivery address line uses &apos;UNIT&apos; followed by the unit identifier, followed by &apos;BOX&apos; followed by box number, in place of a street address, &apos;DPO&apos; as the literal value for the city, and the appropriate armed forces subdivision code in place of a subdivision (state) code</skos:definition>
	</owl:Class>
	
	<owl:Class rdf:about="&fibo-fnd-plc-uspsa;DepartmentOfStateUnitComponent">
		<rdfs:subClassOf rdf:resource="&fibo-fnd-plc-adr;SupplementalAddressComponent"/>
		<rdfs:subClassOf>
			<owl:Restriction>
				<owl:onProperty rdf:resource="&fibo-fnd-rel-rel;comprises"/>
				<owl:hasValue rdf:resource="&fibo-fnd-plc-adr;Unit"/>
			</owl:Restriction>
		</rdfs:subClassOf>
		<rdfs:label>Department of State unit component</rdfs:label>
		<skos:definition>component of a Department of State address that includes &apos;UNIT&apos; followed by the unit identifier</skos:definition>
	</owl:Class>
	
	<owl:NamedIndividual rdf:about="&fibo-fnd-plc-uspsa;East">
		<rdf:type rdf:resource="&fibo-fnd-plc-adr;GeographicDirectionalSymbol"/>
		<rdfs:label xml:lang="en">East</rdfs:label>
		<rdfs:label xml:lang="es">Este</rdfs:label>
		<skos:definition>geographic directional symbol for East</skos:definition>
		<lcc-lr:hasTag>E</lcc-lr:hasTag>
	</owl:NamedIndividual>
	
	<owl:Class rdf:about="&fibo-fnd-plc-uspsa;GeneralDeliveryAddress">
		<rdfs:subClassOf rdf:resource="&fibo-fnd-plc-adr;PhysicalAddress"/>
		<rdfs:subClassOf>
			<owl:Restriction>
				<owl:onProperty rdf:resource="&fibo-fnd-plc-adr;hasAddressLine1"/>
				<owl:hasValue>GENERAL DELIVERY</owl:hasValue>
			</owl:Restriction>
		</rdfs:subClassOf>
		<rdfs:label>general delivery address</rdfs:label>
		<owl:disjointWith rdf:resource="&fibo-fnd-plc-adr;ConventionalStreetAddress"/>
		<skos:definition>delivery address that uses the words &apos;GENERAL DELIVERY&apos;, uppercase preferred, spelled out (no abbreviation), in place of a street address</skos:definition>
		<fibo-fnd-utl-av:explanatoryNote>The value of the +4 component of a ZIP+4 code should be &apos;9999&apos;.</fibo-fnd-utl-av:explanatoryNote>
	</owl:Class>
	
	<owl:Class rdf:about="&fibo-fnd-plc-uspsa;HighwayContractRoute">
		<rdfs:subClassOf rdf:resource="&fibo-fnd-plc-adr;SupplementalAddressComponent"/>
		<rdfs:subClassOf>
			<owl:Restriction>
				<owl:onProperty rdf:resource="&fibo-fnd-rel-rel;comprises"/>
				<owl:hasValue rdf:resource="&fibo-fnd-plc-uspsa;HighwayContractRouteDesignator"/>
			</owl:Restriction>
		</rdfs:subClassOf>
		<rdfs:label>highway contract route</rdfs:label>
		<skos:definition>highway contract route associated with an address</skos:definition>
	</owl:Class>
	
	<owl:Class rdf:about="&fibo-fnd-plc-uspsa;HighwayContractRouteAddress">
		<rdfs:subClassOf rdf:resource="&fibo-fnd-plc-adr;PhysicalAddress"/>
		<rdfs:subClassOf>
			<owl:Restriction>
				<owl:onProperty rdf:resource="&fibo-fnd-rel-rel;comprises"/>
				<owl:onClass rdf:resource="&fibo-fnd-plc-uspsa;HighwayContractRoute"/>
				<owl:qualifiedCardinality rdf:datatype="&xsd;nonNegativeInteger">1</owl:qualifiedCardinality>
			</owl:Restriction>
		</rdfs:subClassOf>
		<rdfs:subClassOf>
			<owl:Restriction>
				<owl:onProperty rdf:resource="&fibo-fnd-rel-rel;comprises"/>
				<owl:onClass rdf:resource="&fibo-fnd-plc-uspsa;Mailbox"/>
				<owl:qualifiedCardinality rdf:datatype="&xsd;nonNegativeInteger">1</owl:qualifiedCardinality>
			</owl:Restriction>
		</rdfs:subClassOf>
		<rdfs:label>highway contract address</rdfs:label>
		<owl:disjointWith rdf:resource="&fibo-fnd-plc-adr;ConventionalStreetAddress"/>
		<skos:definition>delivery address whose delivery address line uses the abbreviation &apos;HC&apos;, followed by the route identifier, followed by &apos;BOX&apos; followed by box number, in place of a street address</skos:definition>
	</owl:Class>
	
	<owl:NamedIndividual rdf:about="&fibo-fnd-plc-uspsa;HighwayContractRouteDesignator">
		<rdf:type rdf:resource="&fibo-fnd-plc-adr;SupplementalAddressDesignator"/>
		<rdfs:label>highway contract route designator</rdfs:label>
		<skos:definition>designator for a route served by an independent contractor rather than directly by the U.S. Postal Service</skos:definition>
		<fibo-fnd-utl-av:preferredDesignation>HC</fibo-fnd-utl-av:preferredDesignation>
	</owl:NamedIndividual>
	
	<owl:Class rdf:about="&fibo-fnd-plc-uspsa;InternationalAddress">
		<rdfs:subClassOf rdf:resource="&fibo-fnd-plc-adr;PhysicalAddress"/>
		<rdfs:label>international address</rdfs:label>
		<owl:equivalentClass>
			<owl:Restriction>
				<owl:onProperty rdf:resource="&fibo-fnd-plc-loc;hasCountry"/>
				<owl:onClass rdf:resource="&lcc-cr;Country"/>
				<owl:qualifiedCardinality rdf:datatype="&xsd;nonNegativeInteger">1</owl:qualifiedCardinality>
			</owl:Restriction>
		</owl:equivalentClass>
		<skos:definition>physical address that explicitly includes a country</skos:definition>
	</owl:Class>
	
	<owl:Class rdf:about="&fibo-fnd-plc-uspsa;Mailbox">
		<rdfs:subClassOf rdf:resource="&fibo-fnd-plc-adr;SupplementalAddressComponent"/>
		<rdfs:subClassOf>
			<owl:Restriction>
				<owl:onProperty rdf:resource="&fibo-fnd-rel-rel;comprises"/>
				<owl:hasValue rdf:resource="&fibo-fnd-plc-uspsa;MailboxDesignator"/>
			</owl:Restriction>
		</rdfs:subClassOf>
		<rdfs:label>mailbox</rdfs:label>
		<skos:definition>mailbox, other than a U.S. Post Office box, associated with an address</skos:definition>
	</owl:Class>
	
	<owl:NamedIndividual rdf:about="&fibo-fnd-plc-uspsa;MailboxDesignator">
		<rdf:type rdf:resource="&fibo-fnd-plc-adr;SupplementalAddressDesignator"/>
		<rdfs:label>mailbox designator</rdfs:label>
		<skos:definition>designator for a mail box other than a U.S. Post Office box</skos:definition>
		<fibo-fnd-utl-av:preferredDesignation>BOX</fibo-fnd-utl-av:preferredDesignation>
	</owl:NamedIndividual>
	
	<owl:NamedIndividual rdf:about="&fibo-fnd-plc-uspsa;North">
		<rdf:type rdf:resource="&fibo-fnd-plc-adr;GeographicDirectionalSymbol"/>
		<rdfs:label xml:lang="es">Norte</rdfs:label>
		<rdfs:label xml:lang="en">North</rdfs:label>
		<skos:definition>geographic directional symbol for North</skos:definition>
		<lcc-lr:hasTag>N</lcc-lr:hasTag>
	</owl:NamedIndividual>
	
	<owl:NamedIndividual rdf:about="&fibo-fnd-plc-uspsa;Northeast">
		<rdf:type rdf:resource="&fibo-fnd-plc-adr;GeographicDirectionalSymbol"/>
		<rdfs:label xml:lang="es">Noreste</rdfs:label>
		<rdfs:label xml:lang="en">Northeast</rdfs:label>
		<skos:definition>geographic directional symbol for Northeast</skos:definition>
		<lcc-lr:hasTag>NE</lcc-lr:hasTag>
	</owl:NamedIndividual>
	
	<owl:NamedIndividual rdf:about="&fibo-fnd-plc-uspsa;Northwest">
		<rdf:type rdf:resource="&fibo-fnd-plc-adr;GeographicDirectionalSymbol"/>
		<rdfs:label xml:lang="es">Noroeste</rdfs:label>
		<rdfs:label xml:lang="en">Northwest</rdfs:label>
		<skos:definition>geographic directional symbol for Northwest</skos:definition>
		<lcc-lr:hasTag>NO</lcc-lr:hasTag>
		<lcc-lr:hasTag>NW</lcc-lr:hasTag>
	</owl:NamedIndividual>
	
	<owl:Class rdf:about="&fibo-fnd-plc-uspsa;OverseasMilitaryAddress">
		<rdfs:subClassOf rdf:resource="&fibo-fnd-plc-adr;PhysicalAddress"/>
		<rdfs:subClassOf>
			<owl:Restriction>
				<owl:onProperty rdf:resource="&fibo-fnd-plc-adr;hasAddressLine1"/>
				<owl:someValuesFrom rdf:resource="&rdfs;Literal"/>
			</owl:Restriction>
		</rdfs:subClassOf>
		<rdfs:subClassOf>
			<owl:Restriction>
				<owl:onProperty rdf:resource="&fibo-fnd-plc-loc;hasCityName"/>
				<owl:someValuesFrom>
					<rdfs:Datatype>
						<owl:oneOf>
							<rdf:Description>
								<rdf:first>APO</rdf:first>
								<rdf:rest>
									<rdf:Description>
										<rdf:first>FPO</rdf:first>
										<rdf:rest rdf:resource="&rdf;nil"/>
									</rdf:Description>
								</rdf:rest>
							</rdf:Description>
						</owl:oneOf>
					</rdfs:Datatype>
				</owl:someValuesFrom>
			</owl:Restriction>
		</rdfs:subClassOf>
		<rdfs:label>overseas military address</rdfs:label>
		<owl:disjointWith rdf:resource="&fibo-fnd-plc-adr;ConventionalStreetAddress"/>
		<skos:definition>delivery address whose delivery address line uses an abbreviation for the unit or command such as &apos;CMR&apos;, &apos;PSC&apos;, or &apos;UNIT&apos;, or  &apos;HC&apos;, followed by the unit identifier, followed by &apos;BOX&apos; followed by box number, in place of a street address, either &apos;APO&apos; or &apos;FPO&apos; as the literal value for the city and the appropriate armed forces subdivision code in place of a subdivision (state) code</skos:definition>
	</owl:Class>
	
	<owl:Class rdf:about="&fibo-fnd-plc-uspsa;PrivateMailBoxAddress">
		<rdfs:subClassOf rdf:resource="&fibo-fnd-plc-adr;ConventionalStreetAddress"/>
		<rdfs:label>private mail box address</rdfs:label>
		<skos:definition>delivery address provided by a commercial mail receiving company that includes a supplementary address line containing the abbreviation &apos;PMB&apos; or the pound &quot;#&quot; symbol followed by the mailbox number; alternatively, &apos;PMB&apos; or &apos;#&quot; and the mailbox number can be appended to the street address</skos:definition>
	</owl:Class>
	
	<owl:Class rdf:about="&fibo-fnd-plc-uspsa;PuertoRicoAddress">
		<rdfs:subClassOf rdf:resource="&fibo-fnd-plc-adr;ConventionalStreetAddress"/>
		<rdfs:subClassOf>
			<owl:Restriction>
				<owl:onProperty rdf:resource="&fibo-fnd-rel-rel;comprises"/>
				<owl:onClass rdf:resource="&fibo-fnd-plc-uspsa;Urbanization"/>
				<owl:minQualifiedCardinality rdf:datatype="&xsd;nonNegativeInteger">0</owl:minQualifiedCardinality>
			</owl:Restriction>
		</rdfs:subClassOf>
		<rdfs:label>Puerto Rico address</rdfs:label>
		<skos:definition>delivery address for a delivery point in Puerto Rico that may include a supplementary address line containing the abbreviation &apos;URB&apos; followed by the name of the urbanization area that is appropriate for that address</skos:definition>
	</owl:Class>
	
	<owl:Class rdf:about="&fibo-fnd-plc-uspsa;RuralRoute">
		<rdfs:subClassOf rdf:resource="&fibo-fnd-plc-adr;SupplementalAddressComponent"/>
		<rdfs:subClassOf>
			<owl:Restriction>
				<owl:onProperty rdf:resource="&fibo-fnd-rel-rel;comprises"/>
				<owl:hasValue rdf:resource="&fibo-fnd-plc-uspsa;RuralRouteDesignator"/>
			</owl:Restriction>
		</rdfs:subClassOf>
		<rdfs:label>highway contract route address</rdfs:label>
		<skos:definition>mail route outside the city or township limits in a rural area associated with an address</skos:definition>
	</owl:Class>
	
	<owl:Class rdf:about="&fibo-fnd-plc-uspsa;RuralRouteAddress">
		<rdfs:subClassOf rdf:resource="&fibo-fnd-plc-adr;PhysicalAddress"/>
		<rdfs:subClassOf>
			<owl:Restriction>
				<owl:onProperty rdf:resource="&fibo-fnd-rel-rel;comprises"/>
				<owl:onClass rdf:resource="&fibo-fnd-plc-uspsa;Mailbox"/>
				<owl:qualifiedCardinality rdf:datatype="&xsd;nonNegativeInteger">1</owl:qualifiedCardinality>
			</owl:Restriction>
		</rdfs:subClassOf>
		<rdfs:subClassOf>
			<owl:Restriction>
				<owl:onProperty rdf:resource="&fibo-fnd-rel-rel;comprises"/>
				<owl:onClass rdf:resource="&fibo-fnd-plc-uspsa;RuralRoute"/>
				<owl:qualifiedCardinality rdf:datatype="&xsd;nonNegativeInteger">1</owl:qualifiedCardinality>
			</owl:Restriction>
		</rdfs:subClassOf>
		<rdfs:label>rural route address</rdfs:label>
		<owl:disjointWith rdf:resource="&fibo-fnd-plc-adr;ConventionalStreetAddress"/>
		<skos:definition>delivery address whose delivery address line uses the abbreviation &apos;RR&apos;, followed by the route identifier, followed by &apos;BOX&apos; followed by box number, in place of a street address</skos:definition>
	</owl:Class>
	
	<owl:NamedIndividual rdf:about="&fibo-fnd-plc-uspsa;RuralRouteDesignator">
		<rdf:type rdf:resource="&fibo-fnd-plc-adr;SupplementalAddressDesignator"/>
		<rdfs:label>rural route designator</rdfs:label>
		<skos:definition>designator for a mail route outside the city or township limits in a rural area</skos:definition>
		<fibo-fnd-utl-av:preferredDesignation>RR</fibo-fnd-utl-av:preferredDesignation>
	</owl:NamedIndividual>
	
	<owl:NamedIndividual rdf:about="&fibo-fnd-plc-uspsa;South">
		<rdf:type rdf:resource="&fibo-fnd-plc-adr;GeographicDirectionalSymbol"/>
		<rdfs:label xml:lang="en">South</rdfs:label>
		<rdfs:label xml:lang="es">Sur</rdfs:label>
		<skos:definition>geographic directional symbol for South</skos:definition>
		<lcc-lr:hasTag>S</lcc-lr:hasTag>
	</owl:NamedIndividual>
	
	<owl:NamedIndividual rdf:about="&fibo-fnd-plc-uspsa;Southeast">
		<rdf:type rdf:resource="&fibo-fnd-plc-adr;GeographicDirectionalSymbol"/>
		<rdfs:label xml:lang="en">Southeast</rdfs:label>
		<rdfs:label xml:lang="es">Sureste</rdfs:label>
		<skos:definition>geographic directional symbol for Southeast</skos:definition>
		<lcc-lr:hasTag>SE</lcc-lr:hasTag>
	</owl:NamedIndividual>
	
	<owl:NamedIndividual rdf:about="&fibo-fnd-plc-uspsa;Southwest">
		<rdf:type rdf:resource="&fibo-fnd-plc-adr;GeographicDirectionalSymbol"/>
		<rdfs:label xml:lang="en">Southwest</rdfs:label>
		<rdfs:label xml:lang="es">Suroeste</rdfs:label>
		<skos:definition>geographic directional symbol for Southwest</skos:definition>
		<lcc-lr:hasTag>SO</lcc-lr:hasTag>
		<lcc-lr:hasTag>SW</lcc-lr:hasTag>
	</owl:NamedIndividual>
	
	<owl:Class rdf:about="&fibo-fnd-plc-uspsa;StandardizedAddress">
		<rdfs:subClassOf rdf:resource="&fibo-fnd-plc-adr;PhysicalAddress"/>
		<rdfs:label>standardized address</rdfs:label>
		<skos:definition>delivery address that is fully spelled out, abbreviated by using the Postal Service standard abbreviations or as given in the current Postal Service ZIP+4 file</skos:definition>
	</owl:Class>
	
	<owl:NamedIndividual rdf:about="&fibo-fnd-plc-uspsa;USPostOfficeBoxDesignator">
		<rdf:type rdf:resource="&fibo-fnd-plc-adr;PostOfficeBoxDesignator"/>
		<rdfs:label>post office box designator</rdfs:label>
		<skos:definition>designator for a U.S. Post Office box</skos:definition>
		<fibo-fnd-utl-av:preferredDesignation>PO BOX</fibo-fnd-utl-av:preferredDesignation>
	</owl:NamedIndividual>
	
	<owl:Class rdf:about="&fibo-fnd-plc-uspsa;USPostalServiceAddressIdentifier">
		<rdfs:subClassOf rdf:resource="&fibo-fnd-plc-adr;PhysicalAddressIdentifier"/>
		<rdfs:subClassOf>
			<owl:Restriction>
				<owl:onProperty rdf:resource="&fibo-fnd-rel-rel;comprises"/>
				<owl:onClass rdf:resource="&fibo-fnd-plc-uspsa;DeliveryPointCode"/>
				<owl:qualifiedCardinality rdf:datatype="&xsd;nonNegativeInteger">1</owl:qualifiedCardinality>
			</owl:Restriction>
		</rdfs:subClassOf>
		<rdfs:subClassOf>
			<owl:Restriction>
				<owl:onProperty rdf:resource="&fibo-fnd-rel-rel;comprises"/>
				<owl:onClass rdf:resource="&fibo-fnd-plc-uspsa;ZIPPlus4Code"/>
				<owl:qualifiedCardinality rdf:datatype="&xsd;nonNegativeInteger">1</owl:qualifiedCardinality>
			</owl:Restriction>
		</rdfs:subClassOf>
		<rdfs:label>U.S. Postal Service address identifier</rdfs:label>
		<skos:definition>combined with the ZIP + 4 code, the delivery point code provides a unique identifier for every deliverable address served by the USPS</skos:definition>
		<fibo-fnd-utl-av:explanatoryNote>The delivery point digits are almost never printed on mail in human-readable form; instead they are encoded in the POSTNET delivery point barcode (DPBC) or as part of the newer Intelligent Mail Barcode (IMB).</fibo-fnd-utl-av:explanatoryNote>
	</owl:Class>
	
	<owl:Class rdf:about="&fibo-fnd-plc-uspsa;Urbanization">
		<rdfs:subClassOf rdf:resource="&lcc-cr;CountrySubdivision"/>
		<rdfs:label>urbanization</rdfs:label>
		<skos:definition>an area, sector, or development within a larger geographic area</skos:definition>
		<fibo-fnd-utl-av:explanatoryNote>This URB descriptor, commonly used in urban areas of Puerto Rico, is an important part of the addressing format, as it describes the location of a given street.</fibo-fnd-utl-av:explanatoryNote>
	</owl:Class>
	
	<owl:NamedIndividual rdf:about="&fibo-fnd-plc-uspsa;West">
		<rdf:type rdf:resource="&fibo-fnd-plc-adr;GeographicDirectionalSymbol"/>
		<rdfs:label xml:lang="es">Oeste</rdfs:label>
		<rdfs:label xml:lang="en">West</rdfs:label>
		<skos:definition>geographic directional symbol for West</skos:definition>
		<lcc-lr:hasTag>O</lcc-lr:hasTag>
		<lcc-lr:hasTag>W</lcc-lr:hasTag>
	</owl:NamedIndividual>
	
	<owl:Class rdf:about="&fibo-fnd-plc-uspsa;ZIPCode">
		<rdfs:subClassOf rdf:resource="&fibo-fnd-plc-adr;Postcode"/>
		<rdfs:label>Zip Code</rdfs:label>
		<skos:definition>five-digit code code assigned to a delivery address indicating the state and post office or postal zone</skos:definition>
	</owl:Class>
	
	<owl:Class rdf:about="&fibo-fnd-plc-uspsa;ZIPPlus4Code">
		<rdfs:subClassOf rdf:resource="&fibo-fnd-plc-adr;Postcode"/>
		<rdfs:label>ZIP+4 Code</rdfs:label>
		<skos:definition>nine-digit number consisting of five digits, a hyphen, and four digits, which the USPS describes by its trademark ZIP+4</skos:definition>
		<fibo-fnd-utl-av:explanatoryNote>The correct format for a numeric ZIP+4 code is five digits, a hyphen, and four digits. The first five digits represent the 5-digit ZIP Code; the sixth and seventh digits (the first two after the hyphen) identify an area known as a sector; the eighth and ninth digits identify a smaller area known as a segment. Together, the final four digits identify geographic units such as a side of a street between intersections, both sides of a street between intersections, a building, a floor or group of floors in a building, a firm within a building, a span of boxes on a rural route, or a group of Post Office boxes to which a single USPS employee makes delivery.</fibo-fnd-utl-av:explanatoryNote>
	</owl:Class>
	
	<owl:Class rdf:about="&fibo-fnd-plc-uspsa;ZipCodeScheme">
		<rdfs:subClassOf rdf:resource="&lcc-lr;CodeSet"/>
		<rdfs:subClassOf rdf:resource="&lcc-lr;IdentificationScheme"/>
		<rdfs:subClassOf>
			<owl:Restriction>
				<owl:onProperty rdf:resource="&lcc-lr;hasMember"/>
				<owl:someValuesFrom>
					<owl:Class>
						<owl:unionOf rdf:parseType="Collection">
							<rdf:Description rdf:about="&fibo-fnd-plc-uspsa;ZIPCode">
							</rdf:Description>
							<rdf:Description rdf:about="&fibo-fnd-plc-uspsa;ZIPPlus4Code">
							</rdf:Description>
						</owl:unionOf>
					</owl:Class>
				</owl:someValuesFrom>
			</owl:Restriction>
		</rdfs:subClassOf>
		<rdfs:label>zip code scheme</rdfs:label>
		<rdfs:seeAlso rdf:resource="https://pe.usps.com/cpim/ftp/pubs/Pub28/pub28.pdf"/>
		<skos:definition>system used in the U.S. to facilitate the delivery of mail, consisting of a five- or nine-digit code Zone Improvement Plan (ZIP) printed directly after the address, the first five digits (initial code) indicating the state and post office or postal zone, the last four (expanded code) the box section or number, portion of a rural route, building, or other specific delivery location</skos:definition>
	</owl:Class>
	
	<owl:ObjectProperty rdf:about="&fibo-fnd-plc-uspsa;hasUrbanization">
		<rdfs:subPropertyOf rdf:resource="&fibo-fnd-rel-rel;comprises"/>
		<rdfs:label>has urbanization</rdfs:label>
		<rdfs:range rdf:resource="&fibo-fnd-plc-uspsa;Urbanization"/>
		<skos:definition>indicates  area, sector, or development within a geographic area relevant to a delivery address</skos:definition>
	</owl:ObjectProperty>

</rdf:RDF>