<?xml version="1.0" encoding="UTF-8"?>
  
<!DOCTYPE rdf:RDF [
    <!ENTITY fibo-der-ctr-exc "http://spec.edmcouncil.org/fibo/red/der/derivatives-contracts/exercise-conventions/">
    <!ENTITY fibo-fnd-pub-stdi "http://spec.edmcouncil.org/fibo/red/fnd/publications/standards-individuals/">
    <!ENTITY fibo-fnd-tim-tim "http://spec.edmcouncil.org/fibo/red/fnd/date-time/date-time/">
    <!ENTITY fibo-der-ctr-opt "http://spec.edmcouncil.org/fibo/red/der/derivatives-contracts/options/">
]>

<rdf:RDF xmlns:xsd="http://www.w3.org/2001/XMLSchema#"
         xmlns:sm="http://www.omg.org/techprocess/ab/SpecificationMetadata/"
         xmlns:xs="http://www.w3.org/2001/XMLSchema"
         xmlns:fibo-fnd-utl-av="http://www.omg.org/spec/EDMC-FIBO/FND/Utilities/AnnotationVocabulary/"
         xmlns:rdf="http://www.w3.org/1999/02/22-rdf-syntax-ns#"
         xmlns:rdfs="http://www.w3.org/2000/01/rdf-schema#"
         xmlns:owl="http://www.w3.org/2002/07/owl#"
         xmlns:skos="http://www.w3.org/2004/02/skos/core#"
         xmlns:dc="http://purl.org/dc/terms/"
         xml:base="http://spec.edmcouncil.org/fibo/red/der/derivatives-contracts/exercise-conventions/">

   <owl:Ontology rdf:about="http://spec.edmcouncil.org/fibo/red/der/derivatives-contracts/exercise-conventions/">
      <owl:imports rdf:resource="http://spec.edmcouncil.org/fibo/red/fnd/publications/standards-individuals/"/>
      <owl:imports rdf:resource="http://spec.edmcouncil.org/fibo/red/fnd/date-time/date-time/"/>
      <owl:imports rdf:resource="http://spec.edmcouncil.org/fibo/red/der/derivatives-contracts/options/"/>
   </owl:Ontology>


  <!--
    ///////////////////////////////////////////////////////////////////////////////////////
    //
    // Datatypes
    //
    ///////////////////////////////////////////////////////////////////////////////////////
    -->



  <!--
    ///////////////////////////////////////////////////////////////////////////////////////
    //
    // Object Properties
    //
    ///////////////////////////////////////////////////////////////////////////////////////
    -->


<owl:ObjectProperty rdf:about="&fibo-der-ctr-exc;exerciseWindow">
      <rdfs:label>exercise window</rdfs:label>
      <skos:definition>The window during which the Exercise can take place.</skos:definition>
      <rdfs:domain rdf:resource="&fibo-der-ctr-exc;AmericanExerciseConvention"/>
      <rdfs:range rdf:resource="&fibo-fnd-tim-tim;DatePeriod"/>
   </owl:ObjectProperty>

   <owl:ObjectProperty rdf:about="&fibo-der-ctr-exc;exerciseDeterminationPeriod">
      <rdfs:label>exercise determination period</rdfs:label>
      <skos:definition>The period during which the value of the underlying i smeasured in order to determine when the option may be exercised. The actual exercise date is the final day of the Exercise Period.</skos:definition>
      <rdfs:domain rdf:resource="&fibo-der-ctr-exc;AsianExerciseCommitment"/>
      <rdfs:range rdf:resource="&fibo-fnd-tim-tim;DatePeriod"/>
   </owl:ObjectProperty>

   <owl:ObjectProperty rdf:about="&fibo-der-ctr-exc;setsOut">
      <rdfs:label>sets out</rdfs:label>
      <rdfs:domain rdf:resource="&fibo-der-ctr-exc;AsianExerciseTermsSet"/>
      <rdfs:range rdf:resource="&fibo-der-ctr-exc;AsianExerciseCommitment"/>
   </owl:ObjectProperty>

   <owl:ObjectProperty rdf:about="&fibo-der-ctr-exc;specifiesExerciseDateConvention">
      <rdfs:label>specifies exercise date convention</rdfs:label>
      <rdfs:subPropertyOf rdf:resource="&fibo-der-ctr-opt;optionExerciseTermsSpecifies"/>
      <rdfs:domain rdf:resource="&fibo-der-ctr-exc;AsianExerciseTermsSet"/>
      <rdfs:range rdf:resource="&fibo-der-ctr-exc;EuropeanExerciseConvention"/>
   </owl:ObjectProperty>

   <owl:ObjectProperty rdf:about="&fibo-der-ctr-exc;exerciseWindow.1">
      <rdfs:label>exercise window</rdfs:label>
      <skos:definition>Each time window during which the Exercise can take place.</skos:definition>
      <rdfs:domain rdf:resource="&fibo-der-ctr-exc;BermudaExerciseConvention"/>
      <rdfs:range rdf:resource="&fibo-fnd-tim-tim;DatePeriod"/>
   </owl:ObjectProperty>


  <!--
    ///////////////////////////////////////////////////////////////////////////////////////
    //
    // Data Properties
    //
    ///////////////////////////////////////////////////////////////////////////////////////
    -->


<owl:DatatypeProperty rdf:about="&fibo-der-ctr-exc;exerciseDate">
      <rdfs:label>exercise date</rdfs:label>
      <skos:definition>The date of exercise (expiry)</skos:definition>
      <rdfs:range rdf:resource="http://www.w3.org/2001/XMLSchema#date"/>
   </owl:DatatypeProperty>


  <!--
    ///////////////////////////////////////////////////////////////////////////////////////
    //
    // Annotation Properties
    //
    ///////////////////////////////////////////////////////////////////////////////////////
    -->



  <!--
    ///////////////////////////////////////////////////////////////////////////////////////
    //
    // Classes
    //
    ///////////////////////////////////////////////////////////////////////////////////////
    -->


<owl:Class rdf:about="&fibo-der-ctr-exc;AmericanExerciseConvention">
      <rdfs:label>american exercise convention</rdfs:label>
      <skos:definition>A feature of an option that stipulates that the option can be exercised anytime within the specified date window.</skos:definition>
      <rdfs:subClassOf rdf:resource="&fibo-der-ctr-exc;ExerciseDatesConvention"/>
   </owl:Class>

   <owl:Class rdf:about="&fibo-der-ctr-exc;AsianExerciseCommitment">
      <rdfs:label>asian exercise commitment</rdfs:label>
      <skos:definition>Commitment to pay out on an option on the basis of a rolling average strike, which the other party may or may not choose to exercise against.</skos:definition>
      <rdfs:subClassOf rdf:resource="&fibo-der-ctr-opt;OptionWriterCommitment"/>
   </owl:Class>

   <owl:Class rdf:about="&fibo-der-ctr-exc;AsianExerciseTermsSet">
      <rdfs:label>asian exercise terms set</rdfs:label>
      <skos:definition>Terms governing the exercise of an Asian Option.</skos:definition>
      <rdfs:subClassOf rdf:resource="&fibo-der-ctr-opt;OptionExerciseTimeTermsSet"/>
   </owl:Class>

   <owl:Class rdf:about="&fibo-der-ctr-exc;BermudaExerciseConvention">
      <rdfs:label>bermuda exercise convention</rdfs:label>
      <skos:definition>A feature of an option that states it can be exercised at different times during the life of the option. The various times set for exercise are written within the option and allow for flexibility for both the writer and holder of the option.</skos:definition>
   </owl:Class>

   <owl:Class rdf:about="&fibo-der-ctr-exc;EuropeanExerciseConvention">
      <rdfs:label>european exercise convention</rdfs:label>
      <skos:definition>A feature of an option that stipulates that the option may only be exercised a stated Exercise Date. Therefore, there can be no early assignment with this type of option.</skos:definition>
   </owl:Class>

   <owl:Class rdf:about="&fibo-der-ctr-exc;ExerciseDatesConvention">
      <rdfs:label>exercise dates convention</rdfs:label>
      <skos:definition>The date terms determining when the holder or future holder of an option can implement the rights defined in the option.</skos:definition>
      <rdfs:subClassOf rdf:resource="&fibo-fnd-pub-stdi;EDMCouncilConvention"/>
   </owl:Class>


  <!--
    ///////////////////////////////////////////////////////////////////////////////////////
    //
    // Individuals
    //
    ///////////////////////////////////////////////////////////////////////////////////////
    -->


</rdf:RDF>