<?xml version="1.0" encoding="UTF-8"?>
  
<!DOCTYPE rdf:RDF [
    <!ENTITY fibo-be-corpx-ceq "http://spec.edmcouncil.org/fibo/red/be/corporations-ext/corporation-equity/">
    <!ENTITY fibo-fnd-law-jur "http://spec.edmcouncil.org/fibo/red/fnd/law/jurisdictions/">
    <!ENTITY fibo-fnd-acc-aeq "http://spec.edmcouncil.org/fibo/red/fnd/accounting/accounting-equity/">
    <!ENTITY fibo-be-oac-exec "http://spec.edmcouncil.org/fibo/red/be/ownership-and-control/executives/">
    <!ENTITY fibo-be-le-cb "http://spec.edmcouncil.org/fibo/red/be/legal-entities/corporate-bodies/">
    <!ENTITY fibo-be-le-fbo "http://spec.edmcouncil.org/fibo/red/be/legal-entities/formal-business-organizations/">
    <!ENTITY fibo-be-corp-corp "http://spec.edmcouncil.org/fibo/red/be/corporations/corporations/">
    <!ENTITY fibo-sec-eq-eqi "http://spec.edmcouncil.org/fibo/red/sec/equities/equity-instruments/">
]>

<rdf:RDF xmlns:xsd="http://www.w3.org/2001/XMLSchema#"
         xmlns:sm="http://www.omg.org/techprocess/ab/SpecificationMetadata/"
         xmlns:xs="http://www.w3.org/2001/XMLSchema"
         xmlns:fibo-fnd-utl-av="http://www.omg.org/spec/EDMC-FIBO/FND/Utilities/AnnotationVocabulary/"
         xmlns:rdf="http://www.w3.org/1999/02/22-rdf-syntax-ns#"
         xmlns:rdfs="http://www.w3.org/2000/01/rdf-schema#"
         xmlns:owl="http://www.w3.org/2002/07/owl#"
         xmlns:skos="http://www.w3.org/2004/02/skos/core#"
         xmlns:dc="http://purl.org/dc/terms/"
         xml:base="http://spec.edmcouncil.org/fibo/red/be/corporations-ext/corporation-equity/">

   <owl:Ontology rdf:about="http://spec.edmcouncil.org/fibo/red/be/corporations-ext/corporation-equity/">
      <owl:imports rdf:resource="http://spec.edmcouncil.org/fibo/red/fnd/law/jurisdictions/"/>
      <owl:imports rdf:resource="http://spec.edmcouncil.org/fibo/red/fnd/accounting/accounting-equity/"/>
      <owl:imports rdf:resource="http://spec.edmcouncil.org/fibo/red/be/ownership-and-control/executives/"/>
      <owl:imports rdf:resource="http://spec.edmcouncil.org/fibo/red/be/legal-entities/corporate-bodies/"/>
      <owl:imports rdf:resource="http://spec.edmcouncil.org/fibo/red/be/legal-entities/formal-business-organizations/"/>
      <owl:imports rdf:resource="http://spec.edmcouncil.org/fibo/red/be/corporations/corporations/"/>
      <owl:imports rdf:resource="http://spec.edmcouncil.org/fibo/red/sec/equities/equity-instruments/"/>
   </owl:Ontology>


  <!--
    ///////////////////////////////////////////////////////////////////////////////////////
    //
    // Datatypes
    //
    ///////////////////////////////////////////////////////////////////////////////////////
    -->



  <!--
    ///////////////////////////////////////////////////////////////////////////////////////
    //
    // Object Properties
    //
    ///////////////////////////////////////////////////////////////////////////////////////
    -->


<owl:ObjectProperty rdf:about="&fibo-be-corpx-ceq;owns">
      <rdfs:label>owns</rdfs:label>
      <skos:definition>Publicly issued equity in a company incorporated by shares, owned by the business entity.</skos:definition>
      <rdfs:subPropertyOf rdf:resource="&fibo-be-corpx-ceq;owns.1"/>
      <rdfs:domain rdf:resource="&fibo-be-le-fbo;FormallyConstitutedOrganization"/>
      <rdfs:range rdf:resource="&fibo-sec-eq-eqi;PubliclyIssuedEquity"/>
   </owl:ObjectProperty>

   <owl:ObjectProperty rdf:about="&fibo-be-corpx-ceq;owns.1">
      <rdfs:label>owns</rdfs:label>
      <skos:definition>Equity in a company incorporated by shares, owned privately or publicly by the business entity.</skos:definition>
      <rdfs:domain rdf:resource="&fibo-be-le-fbo;FormallyConstitutedOrganization"/>
      <rdfs:range rdf:resource="&fibo-fnd-acc-aeq;StockholdersEquity"/>
   </owl:ObjectProperty>

   <owl:ObjectProperty rdf:about="&fibo-be-corpx-ceq;governingLaw">
      <rdfs:label>governing law</rdfs:label>
      <skos:definition>The Jurisdiction in which the Company Legal Form is defined.</skos:definition>
      <rdfs:domain rdf:resource="&fibo-be-oac-exec;ArticlesOfIncorporation"/>
      <rdfs:range rdf:resource="&fibo-fnd-law-jur;Jurisdiction"/>
   </owl:ObjectProperty>

   <owl:ObjectProperty rdf:about="&fibo-be-corpx-ceq;governedBy">
      <rdfs:label>governed by</rdfs:label>
      <skos:definition>The Company constitution or Articles of Inforporation, Articles of Association etc. which defines the terms for equity instruments issued by that company.</skos:definition>
      <rdfs:domain rdf:resource="&fibo-sec-eq-eqi;Share"/>
      <rdfs:range rdf:resource="&fibo-be-oac-exec;ArticlesOfIncorporation"/>
   </owl:ObjectProperty>

   <owl:ObjectProperty rdf:about="&fibo-be-corpx-ceq;hasMajorityHoldingOfAnotherCompanys">
      <rdfs:label>has majority holding of another companys</rdfs:label>
      <skos:definition>Majority Equity held by the company, in another company. This is assumed to be publicly issued equity.</skos:definition>
      <rdfs:subPropertyOf rdf:resource="&fibo-be-corpx-ceq;hasHoldingOfAnotherCompanys"/>
      <rdfs:domain rdf:resource="&fibo-be-corp-corp;IncorporatedCompany"/>
      <rdfs:range rdf:resource="&fibo-sec-eq-eqi;PubliclyIssuedEquity"/>
   </owl:ObjectProperty>

   <owl:ObjectProperty rdf:about="&fibo-be-corpx-ceq;hasHoldingOfAnotherCompanys">
      <rdfs:label>has holding of another companys</rdfs:label>
      <skos:definition>Equity held by the company, in another company. This is assumed to be publicly issued equity.</skos:definition>
      <rdfs:subPropertyOf rdf:resource="&fibo-be-corpx-ceq;owns"/>
      <rdfs:domain rdf:resource="&fibo-be-corp-corp;IncorporatedCompany"/>
      <rdfs:range rdf:resource="&fibo-sec-eq-eqi;PubliclyIssuedEquity"/>
   </owl:ObjectProperty>

   <owl:ObjectProperty rdf:about="&fibo-be-corpx-ceq;hasCapital">
      <rdfs:label>has capital</rdfs:label>
      <skos:definition>The capital issued by the company at its formation or subsequently.</skos:definition>
      <rdfs:subPropertyOf rdf:resource="&fibo-be-corpx-ceq;hasCapital.2"/>
      <rdfs:domain rdf:resource="&fibo-be-corp-corp;PrivatelyHeldCompany"/>
      <rdfs:range rdf:resource="&fibo-sec-eq-eqi;PrivateEquity"/>
   </owl:ObjectProperty>

   <owl:ObjectProperty rdf:about="&fibo-be-corpx-ceq;hasCapital.1">
      <rdfs:label>has capital</rdfs:label>
      <skos:definition>Capital issued publicly by the company and held by the public.</skos:definition>
      <rdfs:subPropertyOf rdf:resource="&fibo-be-corpx-ceq;hasCapital.2"/>
      <rdfs:domain rdf:resource="&fibo-be-corp-corp;PubliclyHeldCompany"/>
      <rdfs:range rdf:resource="&fibo-sec-eq-eqi;PubliclyIssuedEquity"/>
   </owl:ObjectProperty>

   <owl:ObjectProperty rdf:about="&fibo-be-corpx-ceq;mayHaveCapitalAs">
      <rdfs:label>may have capital as</rdfs:label>
      <skos:definition>Additional privately held equity in the company, which is not held as publicly issued shares.</skos:definition>
      <rdfs:subPropertyOf rdf:resource="&fibo-be-corpx-ceq;hasCapital.2"/>
      <rdfs:domain rdf:resource="&fibo-be-corp-corp;PubliclyHeldCompany"/>
      <rdfs:range rdf:resource="&fibo-sec-eq-eqi;PrivateEquity"/>
   </owl:ObjectProperty>

   <owl:ObjectProperty rdf:about="&fibo-be-corpx-ceq;setOutIn">
      <rdfs:label>set out in</rdfs:label>
      <rdfs:domain rdf:resource="&fibo-sec-eq-eqi;VotingRight"/>
      <rdfs:range rdf:resource="&fibo-be-oac-exec;ArticlesOfIncorporation"/>
   </owl:ObjectProperty>

   <owl:ObjectProperty rdf:about="&fibo-be-corpx-ceq;hasCapital.2">
      <rdfs:label>has capital</rdfs:label>
      <skos:definition>The capital issued by the company at its formation or subsequently.</skos:definition>
      <rdfs:subPropertyOf rdf:resource="&fibo-be-le-cb;issuesEquity"/>
      <rdfs:domain rdf:resource="&fibo-be-corp-corp;IncorporatedCompany"/>
      <rdfs:range rdf:resource="&fibo-sec-eq-eqi;ShareholderEquity"/>
   </owl:ObjectProperty>


  <!--
    ///////////////////////////////////////////////////////////////////////////////////////
    //
    // Data Properties
    //
    ///////////////////////////////////////////////////////////////////////////////////////
    -->



  <!--
    ///////////////////////////////////////////////////////////////////////////////////////
    //
    // Annotation Properties
    //
    ///////////////////////////////////////////////////////////////////////////////////////
    -->



  <!--
    ///////////////////////////////////////////////////////////////////////////////////////
    //
    // Classes
    //
    ///////////////////////////////////////////////////////////////////////////////////////
    -->



  <!--
    ///////////////////////////////////////////////////////////////////////////////////////
    //
    // Individuals
    //
    ///////////////////////////////////////////////////////////////////////////////////////
    -->


</rdf:RDF>