<?xml version="1.0" encoding="UTF-8"?>
  
<!DOCTYPE rdf:RDF [
    <!ENTITY fibo-der-etd-dst "http://spec.edmcouncil.org/fibo/red/der/exchange-traded-derivatives/derivatives-standardized-terms/">
    <!ENTITY fibo-fnd-bus-ser "http://spec.edmcouncil.org/fibo/red/fnd/business/services/">
    <!ENTITY fibo-fnd-utl-bt "http://spec.edmcouncil.org/fibo/red/fnd/utilities/business-facing-types/">
    <!ENTITY fibo-der-etd-ost "http://spec.edmcouncil.org/fibo/red/der/exchange-traded-derivatives/options-standardized-terms/">
    <!ENTITY fibo-sec-sec-lst "http://spec.edmcouncil.org/fibo/red/sec/securities/securities-listings/">
]>

<rdf:RDF xmlns:xsd="http://www.w3.org/2001/XMLSchema#"
         xmlns:sm="http://www.omg.org/techprocess/ab/SpecificationMetadata/"
         xmlns:xs="http://www.w3.org/2001/XMLSchema"
         xmlns:fibo-fnd-utl-av="http://www.omg.org/spec/EDMC-FIBO/FND/Utilities/AnnotationVocabulary/"
         xmlns:rdf="http://www.w3.org/1999/02/22-rdf-syntax-ns#"
         xmlns:rdfs="http://www.w3.org/2000/01/rdf-schema#"
         xmlns:owl="http://www.w3.org/2002/07/owl#"
         xmlns:skos="http://www.w3.org/2004/02/skos/core#"
         xmlns:dc="http://purl.org/dc/terms/"
         xml:base="http://spec.edmcouncil.org/fibo/red/der/exchange-traded-derivatives/derivatives-standardized-terms/">

   <owl:Ontology rdf:about="http://spec.edmcouncil.org/fibo/red/der/exchange-traded-derivatives/derivatives-standardized-terms/">
      <owl:imports rdf:resource="http://spec.edmcouncil.org/fibo/red/fnd/business/services/"/>
      <owl:imports rdf:resource="http://spec.edmcouncil.org/fibo/red/fnd/utilities/business-facing-types/"/>
      <owl:imports rdf:resource="http://spec.edmcouncil.org/fibo/red/der/exchange-traded-derivatives/options-standardized-terms/"/>
      <owl:imports rdf:resource="http://spec.edmcouncil.org/fibo/red/sec/securities/securities-listings/"/>
   </owl:Ontology>


  <!--
    ///////////////////////////////////////////////////////////////////////////////////////
    //
    // Datatypes
    //
    ///////////////////////////////////////////////////////////////////////////////////////
    -->


<rdfs:Datatype rdf:about="&fibo-der-etd-dst;DerivativesDeliveryTypeSelection">
      <skos:definition>Type of delivery for a traded futures or options contract; the way in which a contract is settled in the event of expiry or exercise.</skos:definition>
      <owl:equivalentClass>
         <rdfs:Datatype>
            <owl:oneOf>
               <rdf:Description>
                  <rdf:first rdf:datatype="http://www.w3.org/2001/XMLSchema#string">Cash</rdf:first>
                  <rdf:rest>
                     <rdf:Description>
                        <rdf:first rdf:datatype="http://www.w3.org/2001/XMLSchema#string">Squaring Off</rdf:first>
                        <rdf:rest>
                           <rdf:Description>
                              <rdf:first rdf:datatype="http://www.w3.org/2001/XMLSchema#string">Physical</rdf:first>
                              <rdf:rest rdf:resource="http://www.w3.org/1999/02/22-rdf-syntax-ns#nil"/>
                           </rdf:Description>
                        </rdf:rest>
                     </rdf:Description>
                  </rdf:rest>
               </rdf:Description>
            </owl:oneOf>
         </rdfs:Datatype>
      </owl:equivalentClass>
   </rdfs:Datatype>

   <rdfs:Datatype rdf:about="&fibo-der-etd-dst;DerivativesPriceDeterminationMethodSelection">
      <skos:definition>Method by which prices are arrived at for derivatives securities (futures or options).</skos:definition>
      <owl:equivalentClass>
         <rdfs:Datatype>
            <owl:oneOf>
               <rdf:Description>
                  <rdf:first rdf:datatype="http://www.w3.org/2001/XMLSchema#string">Open Outcry</rdf:first>
                  <rdf:rest>
                     <rdf:Description>
                        <rdf:first rdf:datatype="http://www.w3.org/2001/XMLSchema#string">Electronic</rdf:first>
                        <rdf:rest rdf:resource="http://www.w3.org/1999/02/22-rdf-syntax-ns#nil"/>
                     </rdf:Description>
                  </rdf:rest>
               </rdf:Description>
            </owl:oneOf>
         </rdfs:Datatype>
      </owl:equivalentClass>
   </rdfs:Datatype>


  <!--
    ///////////////////////////////////////////////////////////////////////////////////////
    //
    // Object Properties
    //
    ///////////////////////////////////////////////////////////////////////////////////////
    -->


<owl:ObjectProperty rdf:about="&fibo-der-etd-dst;providedBy">
      <rdfs:label>provided by</rdfs:label>
      <rdfs:subPropertyOf rdf:resource="&fibo-fnd-bus-ser;providedBy"/>
      <rdfs:domain rdf:resource="&fibo-der-etd-dst;DerivativesClearing"/>
      <rdfs:range rdf:resource="&fibo-der-etd-dst;.UnionClass.3"/>
   </owl:ObjectProperty>


  <!--
    ///////////////////////////////////////////////////////////////////////////////////////
    //
    // Data Properties
    //
    ///////////////////////////////////////////////////////////////////////////////////////
    -->


<owl:DatatypeProperty rdf:about="&fibo-der-etd-dst;evenLotSize">
      <rdfs:label>even lot size</rdfs:label>
      <skos:definition>Unit of trading in a commodity, established by an exchange, and to which official price quotations from that exchange apply.</skos:definition>
      <rdfs:range rdf:resource="&fibo-fnd-utl-bt;wholeNumber"/>
   </owl:DatatypeProperty>

   <owl:DatatypeProperty rdf:about="&fibo-der-etd-dst;openOutcry">
      <rdfs:label>open outcry</rdfs:label>
      <skos:definition>Whether trading on the exchange is by way of open outcry in the form of physical interaction between participants. No means that trading is carried out electronically.</skos:definition>
      <rdfs:range rdf:resource="&fibo-fnd-utl-bt;yesOrNo"/>
   </owl:DatatypeProperty>


  <!--
    ///////////////////////////////////////////////////////////////////////////////////////
    //
    // Annotation Properties
    //
    ///////////////////////////////////////////////////////////////////////////////////////
    -->



  <!--
    ///////////////////////////////////////////////////////////////////////////////////////
    //
    // Classes
    //
    ///////////////////////////////////////////////////////////////////////////////////////
    -->


<owl:Class rdf:about="&fibo-der-etd-dst;.UnionClass.3">
      <skos:definition>Either a derivatives exchange or an options clearing entity.</skos:definition>
      <owl:equivalentClass>
         <owl:Class>
            <owl:unionOf rdf:parseType="Collection">
               <owl:Class rdf:about="&fibo-der-etd-ost;OptionsClearingEntity"/>
               <owl:Class rdf:about="&fibo-der-etd-dst;DerivativesExchange"/>
            </owl:unionOf>
         </owl:Class>
      </owl:equivalentClass>
   </owl:Class>

   <owl:Class rdf:about="&fibo-der-etd-dst;DerivativesClearing">
      <rdfs:label>derivatives clearing</rdfs:label>
      <skos:definition>The service... This is correect - this role applies the same to Futures and Options contracts on derivatives exchanges. This is always on a Futures Exchange. There are similar terms / facilities for options traded on a Stock Exchange. Also American v European by implication of the nature of the underlying i.e. whether it's a stock or a futures contract.</skos:definition>
      <rdfs:subClassOf rdf:resource="&fibo-der-etd-dst;DerivativesListing"/>
   </owl:Class>

   <owl:Class rdf:about="&fibo-der-etd-dst;DerivativesExchange">
      <rdfs:label>derivatives exchange</rdfs:label>
      <skos:definition>Exchange where futures contracts and options on futures contracts are traded.</skos:definition>
      <rdfs:subClassOf rdf:resource="&fibo-sec-sec-lst;SecuritiesTradingFacility"/>
   </owl:Class>

   <owl:Class rdf:about="&fibo-der-etd-dst;DerivativesListing">
      <rdfs:label>derivatives listing</rdfs:label>
      <skos:definition>A listing of an instrument on a derivatives exchange. The listing is a product of the individual exchange.</skos:definition>
      <rdfs:subClassOf rdf:resource="&fibo-fnd-bus-ser;MarketplaceService"/>
   </owl:Class>


  <!--
    ///////////////////////////////////////////////////////////////////////////////////////
    //
    // Individuals
    //
    ///////////////////////////////////////////////////////////////////////////////////////
    -->


</rdf:RDF>