<?xml version="1.0" encoding="UTF-8"?>
  
<!DOCTYPE rdf:RDF [
    <!ENTITY fibo-sec-sec-id "http://spec.edmcouncil.org/fibo/red/sec/securities/securities-identification/">
    <!ENTITY fibo-fnd-info-ids "http://spec.edmcouncil.org/fibo/red/fnd/information/identifiers/">
    <!ENTITY fibo-sec-sec-iss "http://spec.edmcouncil.org/fibo/red/sec/securities/securities-issuance-terms/">
    <!ENTITY fibo-sec-sec-sec "http://spec.edmcouncil.org/fibo/red/sec/securities/securities/">
    <!ENTITY fibo-sec-sec-ind "http://spec.edmcouncil.org/fibo/red/sec/securities/securities-identification-individuals/">
]>

<rdf:RDF xmlns:xsd="http://www.w3.org/2001/XMLSchema#"
         xmlns:sm="http://www.omg.org/techprocess/ab/SpecificationMetadata/"
         xmlns:xs="http://www.w3.org/2001/XMLSchema"
         xmlns:fibo-fnd-utl-av="http://www.omg.org/spec/EDMC-FIBO/FND/Utilities/AnnotationVocabulary/"
         xmlns:rdf="http://www.w3.org/1999/02/22-rdf-syntax-ns#"
         xmlns:rdfs="http://www.w3.org/2000/01/rdf-schema#"
         xmlns:owl="http://www.w3.org/2002/07/owl#"
         xmlns:skos="http://www.w3.org/2004/02/skos/core#"
         xmlns:dc="http://purl.org/dc/terms/"
         xml:base="http://spec.edmcouncil.org/fibo/red/sec/securities/securities-identification/">

   <owl:Ontology rdf:about="http://spec.edmcouncil.org/fibo/red/sec/securities/securities-identification/">
      <owl:imports rdf:resource="http://spec.edmcouncil.org/fibo/red/fnd/information/identifiers/"/>
      <owl:imports rdf:resource="http://spec.edmcouncil.org/fibo/red/sec/securities/securities-issuance-terms/"/>
      <owl:imports rdf:resource="http://spec.edmcouncil.org/fibo/red/sec/securities/securities/"/>
      <owl:imports rdf:resource="http://spec.edmcouncil.org/fibo/red/sec/securities/securities-identification-individuals/"/>
   </owl:Ontology>


  <!--
    ///////////////////////////////////////////////////////////////////////////////////////
    //
    // Datatypes
    //
    ///////////////////////////////////////////////////////////////////////////////////////
    -->



  <!--
    ///////////////////////////////////////////////////////////////////////////////////////
    //
    // Object Properties
    //
    ///////////////////////////////////////////////////////////////////////////////////////
    -->


<owl:ObjectProperty rdf:about="&fibo-sec-sec-id;definedInScheme">
      <rdfs:label>defined in scheme</rdfs:label>
      <rdfs:subPropertyOf rdf:resource="&fibo-sec-sec-id;definedIn"/>
      <rdfs:domain rdf:resource="&fibo-sec-sec-id;ListedSecurityIdentifier"/>
      <rdfs:range rdf:resource="&fibo-sec-sec-id;ExchangeSecurityIdentificationScheme"/>
   </owl:ObjectProperty>

   <owl:ObjectProperty rdf:about="&fibo-sec-sec-id;hasNationalIdentifier">
      <rdfs:label>has national identifier</rdfs:label>
      <rdfs:subPropertyOf rdf:resource="&fibo-sec-sec-id;hasSecurityIdentifier"/>
      <rdfs:domain rdf:resource="&fibo-sec-sec-sec;ExchangeTradedSecurity"/>
      <rdfs:range rdf:resource="&fibo-sec-sec-id;NationalNumberingAgencyIdentificationCode"/>
   </owl:ObjectProperty>

   <owl:ObjectProperty rdf:about="&fibo-sec-sec-id;hasIdentifier">
      <rdfs:label>has identifier</rdfs:label>
      <rdfs:subPropertyOf rdf:resource="&fibo-sec-sec-id;hasSecurityIdentifier"/>
      <rdfs:domain rdf:resource="&fibo-sec-sec-iss;OfferIssue"/>
      <rdfs:range rdf:resource="&fibo-sec-sec-id;ListedSecurityIdentifier"/>
   </owl:ObjectProperty>

   <owl:ObjectProperty rdf:about="&fibo-sec-sec-id;canBecomePartOf">
      <rdfs:label>can become part of</rdfs:label>
      <skos:definition>A national identification code may become part of a more general identification code (for example, ISIN).</skos:definition>
      <rdfs:domain rdf:resource="&fibo-sec-sec-id;NationalNumberingAgencyIdentificationCode"/>
      <rdfs:range rdf:resource="&fibo-sec-sec-id;SecurityIdentifier"/>
   </owl:ObjectProperty>

   <owl:ObjectProperty rdf:about="&fibo-sec-sec-id;becomesPartOf">
      <rdfs:label>becomes part of</rdfs:label>
      <rdfs:subPropertyOf rdf:resource="&fibo-sec-sec-id;canBecomePartOf"/>
      <rdfs:domain rdf:resource="&fibo-sec-sec-id;NationalNumberingAgencyIdentificationCode"/>
      <rdfs:range rdf:resource="&fibo-sec-sec-ind;ISINIdentifier"/>
   </owl:ObjectProperty>

   <owl:ObjectProperty rdf:about="&fibo-sec-sec-id;definedInScheme.1">
      <rdfs:label>defined in scheme</rdfs:label>
      <rdfs:subPropertyOf rdf:resource="&fibo-sec-sec-id;definedIn"/>
      <rdfs:domain rdf:resource="&fibo-sec-sec-id;NationalNumberingAgencyIdentificationCode"/>
      <rdfs:range rdf:resource="&fibo-sec-sec-id;NationalSecurityIdentificationScheme"/>
   </owl:ObjectProperty>

   <owl:ObjectProperty rdf:about="&fibo-sec-sec-id;definedInScheme.2">
      <rdfs:label>defined in scheme</rdfs:label>
      <rdfs:subPropertyOf rdf:resource="&fibo-sec-sec-id;definedIn"/>
      <rdfs:domain rdf:resource="&fibo-sec-sec-id;ProprietarySecurityIdentificationCode"/>
      <rdfs:range rdf:resource="&fibo-sec-sec-id;ProprietarySecurityIdentificationScheme"/>
   </owl:ObjectProperty>

   <owl:ObjectProperty rdf:about="&fibo-sec-sec-id;defines">
      <rdfs:label>defines</rdfs:label>
      <rdfs:subPropertyOf rdf:resource="&fibo-fnd-info-ids;defines"/>
      <rdfs:domain rdf:resource="&fibo-sec-sec-id;SecurityIdentificationScheme"/>
      <rdfs:range rdf:resource="&fibo-sec-sec-id;SecurityIdentifier"/>
   </owl:ObjectProperty>

   <owl:ObjectProperty rdf:about="&fibo-sec-sec-id;definedIn">
      <rdfs:label>defined in</rdfs:label>
      <rdfs:subPropertyOf rdf:resource="&fibo-fnd-info-ids;definedIn"/>
      <rdfs:domain rdf:resource="&fibo-sec-sec-id;SecurityIdentifier"/>
      <rdfs:range rdf:resource="&fibo-sec-sec-id;SecurityIdentificationScheme"/>
      <owl:inverseOf rdf:resource="&fibo-sec-sec-id;defines"/>
   </owl:ObjectProperty>

   <owl:ObjectProperty rdf:about="&fibo-sec-sec-id;hasSecurityIdentifier">
      <rdfs:label>has security identifier</rdfs:label>
      <skos:definition>The primary identification code of the security. This may be any publicly defined code that is used to identify the Security.</skos:definition>
      <rdfs:subPropertyOf rdf:resource="&fibo-fnd-info-ids;hasIdentifier"/>
      <rdfs:domain rdf:resource="&fibo-sec-sec-sec;Security"/>
      <rdfs:range rdf:resource="&fibo-sec-sec-id;SecurityIdentifier"/>
   </owl:ObjectProperty>


  <!--
    ///////////////////////////////////////////////////////////////////////////////////////
    //
    // Data Properties
    //
    ///////////////////////////////////////////////////////////////////////////////////////
    -->



  <!--
    ///////////////////////////////////////////////////////////////////////////////////////
    //
    // Annotation Properties
    //
    ///////////////////////////////////////////////////////////////////////////////////////
    -->



  <!--
    ///////////////////////////////////////////////////////////////////////////////////////
    //
    // Classes
    //
    ///////////////////////////////////////////////////////////////////////////////////////
    -->


<owl:Class rdf:about="&fibo-sec-sec-id;ExchangeSecurityIdentificationScheme">
      <rdfs:label>exchange security identification scheme</rdfs:label>
      <skos:definition>An identification scheme used by a securities exchange in issuing security identifiers.</skos:definition>
      <rdfs:subClassOf rdf:resource="&fibo-sec-sec-id;SecurityIdentificationScheme"/>
   </owl:Class>

   <owl:Class rdf:about="&fibo-sec-sec-id;ListedSecurityIdentifier">
      <rdfs:label>listed security identifier</rdfs:label>
      <skos:definition>A Security Identifier issued in the public domain and referred to in listings etc.</skos:definition>
      <rdfs:subClassOf rdf:resource="&fibo-sec-sec-id;SecurityIdentifier"/>
   </owl:Class>

   <owl:Class rdf:about="&fibo-sec-sec-id;NationalNumberingAgencyIdentificationCode">
      <rdfs:label>national numbering agency identification code</rdfs:label>
      <skos:definition>An identifier assigned by a national numbering agency under the ISO 6166 standard.</skos:definition>
   </owl:Class>

   <owl:Class rdf:about="&fibo-sec-sec-id;NationalSecurityIdentificationScheme">
      <rdfs:label>national security identification scheme</rdfs:label>
      <skos:definition>A security identification scheme published nationally on behalf of a whole country. Generally incorporated into the ISIN scheme as well.</skos:definition>
   </owl:Class>

   <owl:Class rdf:about="&fibo-sec-sec-id;ProprietarySecurityIdentificationCode">
      <rdfs:label>proprietary security identification code</rdfs:label>
      <skos:definition>An identifier supplied by a commercial data providers or governments, for example a RIC code.</skos:definition>
   </owl:Class>

   <owl:Class rdf:about="&fibo-sec-sec-id;ProprietarySecurityIdentificationScheme">
      <rdfs:label>proprietary security identification scheme</rdfs:label>
      <skos:definition>A security identification format published by a data provider or other commercial entity.</skos:definition>
   </owl:Class>

   <owl:Class rdf:about="&fibo-sec-sec-id;SecurityIdentificationScheme">
      <rdfs:label>security identification scheme</rdfs:label>
      <skos:definition>A formal definition of the structure and application of a particular set of securities identifiers.</skos:definition>
      <rdfs:subClassOf rdf:resource="&fibo-fnd-info-ids;IdentificationScheme"/>
   </owl:Class>

   <owl:Class rdf:about="&fibo-sec-sec-id;SecurityIdentifier">
      <rdfs:label>security identifier</rdfs:label>
      <skos:definition>Any publicly defined code that is used to identify a Security.</skos:definition>
      <rdfs:subClassOf rdf:resource="&fibo-fnd-info-ids;Identifier"/>
   </owl:Class>


  <!--
    ///////////////////////////////////////////////////////////////////////////////////////
    //
    // Individuals
    //
    ///////////////////////////////////////////////////////////////////////////////////////
    -->


</rdf:RDF>