<?xml version="1.0" encoding="UTF-8"?>
  
<!DOCTYPE rdf:RDF [
    <!ENTITY fibo-sec-sec-rst "http://spec.edmcouncil.org/fibo/red/sec/securities/securities-restrictions/">
    <!ENTITY fibo-fnd-lawx-rst "http://spec.edmcouncil.org/fibo/red/fnd/law-ext/restrictions/">
    <!ENTITY fibo-fnd-law-jur "http://spec.edmcouncil.org/fibo/red/fnd/law/jurisdictions/">
    <!ENTITY fibo-fnd-plcx-gpli "http://spec.edmcouncil.org/fibo/red/fnd/places-ext/geopolitical-usa/">
    <!ENTITY fibo-bp-reg-reg "http://spec.edmcouncil.org/fibo/red/bp/regulatory/regulatory-requirements/">
    <!ENTITY fibo-fnd-utl-bt "http://spec.edmcouncil.org/fibo/red/fnd/utilities/business-facing-types/">
    <!ENTITY fibo-sec-sec-sec "http://spec.edmcouncil.org/fibo/red/sec/securities/securities/">
    <!ENTITY fibo-sec-sec-fi "http://spec.edmcouncil.org/fibo/red/sec/securities/financial-instruments/">
    <!ENTITY fibo-fnd-tim-tim "http://spec.edmcouncil.org/fibo/red/fnd/date-time/date-time/">
]>

<rdf:RDF xmlns:xsd="http://www.w3.org/2001/XMLSchema#"
         xmlns:sm="http://www.omg.org/techprocess/ab/SpecificationMetadata/"
         xmlns:xs="http://www.w3.org/2001/XMLSchema"
         xmlns:fibo-fnd-utl-av="http://www.omg.org/spec/EDMC-FIBO/FND/Utilities/AnnotationVocabulary/"
         xmlns:rdf="http://www.w3.org/1999/02/22-rdf-syntax-ns#"
         xmlns:rdfs="http://www.w3.org/2000/01/rdf-schema#"
         xmlns:owl="http://www.w3.org/2002/07/owl#"
         xmlns:skos="http://www.w3.org/2004/02/skos/core#"
         xmlns:dc="http://purl.org/dc/terms/"
         xml:base="http://spec.edmcouncil.org/fibo/red/sec/securities/securities-restrictions/">

   <owl:Ontology rdf:about="http://spec.edmcouncil.org/fibo/red/sec/securities/securities-restrictions/">
      <owl:imports rdf:resource="http://spec.edmcouncil.org/fibo/red/fnd/law-ext/restrictions/"/>
      <owl:imports rdf:resource="http://spec.edmcouncil.org/fibo/red/fnd/law/jurisdictions/"/>
      <owl:imports rdf:resource="http://spec.edmcouncil.org/fibo/red/fnd/places-ext/geopolitical-usa/"/>
      <owl:imports rdf:resource="http://spec.edmcouncil.org/fibo/red/bp/regulatory/regulatory-requirements/"/>
      <owl:imports rdf:resource="http://spec.edmcouncil.org/fibo/red/fnd/utilities/business-facing-types/"/>
      <owl:imports rdf:resource="http://spec.edmcouncil.org/fibo/red/sec/securities/securities/"/>
      <owl:imports rdf:resource="http://spec.edmcouncil.org/fibo/red/sec/securities/financial-instruments/"/>
      <owl:imports rdf:resource="http://spec.edmcouncil.org/fibo/red/fnd/date-time/date-time/"/>
   </owl:Ontology>


  <!--
    ///////////////////////////////////////////////////////////////////////////////////////
    //
    // Datatypes
    //
    ///////////////////////////////////////////////////////////////////////////////////////
    -->


<rdfs:Datatype rdf:about="&fibo-sec-sec-rst;InvestorDomicileType">
      <skos:definition>The type of an Investor, for example for use in defining a Restriction on Holders.</skos:definition>
      <owl:equivalentClass>
         <rdfs:Datatype>
            <owl:oneOf>
               <rdf:Description>
                  <rdf:first rdf:datatype="http://www.w3.org/2001/XMLSchema#string">Citizen</rdf:first>
                  <rdf:rest>
                     <rdf:Description>
                        <rdf:first rdf:datatype="http://www.w3.org/2001/XMLSchema#string">Legal Resident</rdf:first>
                        <rdf:rest>
                           <rdf:Description>
                              <rdf:first rdf:datatype="http://www.w3.org/2001/XMLSchema#string">Individual</rdf:first>
                              <rdf:rest rdf:resource="http://www.w3.org/1999/02/22-rdf-syntax-ns#nil"/>
                           </rdf:Description>
                        </rdf:rest>
                     </rdf:Description>
                  </rdf:rest>
               </rdf:Description>
            </owl:oneOf>
         </rdfs:Datatype>
      </owl:equivalentClass>
   </rdfs:Datatype>

   <rdfs:Datatype rdf:about="&fibo-sec-sec-rst;InvestorType">
      <skos:definition>Type of Investor, in terms of their role and standing (as distinct from residency or citizenship status).</skos:definition>
      <owl:equivalentClass>
         <rdfs:Datatype>
            <owl:oneOf>
               <rdf:Description>
                  <rdf:first rdf:datatype="http://www.w3.org/2001/XMLSchema#string">Physical Person</rdf:first>
                  <rdf:rest>
                     <rdf:Description>
                        <rdf:first rdf:datatype="http://www.w3.org/2001/XMLSchema#string">Staff</rdf:first>
                        <rdf:rest>
                           <rdf:Description>
                              <rdf:first rdf:datatype="http://www.w3.org/2001/XMLSchema#string">Retail</rdf:first>
                              <rdf:rest>
                                 <rdf:Description>
                                    <rdf:first rdf:datatype="http://www.w3.org/2001/XMLSchema#string">Professional</rdf:first>
                                    <rdf:rest rdf:resource="http://www.w3.org/1999/02/22-rdf-syntax-ns#nil"/>
                                 </rdf:Description>
                              </rdf:rest>
                           </rdf:Description>
                        </rdf:rest>
                     </rdf:Description>
                  </rdf:rest>
               </rdf:Description>
            </owl:oneOf>
         </rdfs:Datatype>
      </owl:equivalentClass>
   </rdfs:Datatype>


  <!--
    ///////////////////////////////////////////////////////////////////////////////////////
    //
    // Object Properties
    //
    ///////////////////////////////////////////////////////////////////////////////////////
    -->


<owl:ObjectProperty rdf:about="&fibo-sec-sec-rst;notClearedIn">
      <rdfs:label>not cleared in</rdfs:label>
      <skos:definition>List of the states where issue is NOT cleared under Blue Sky Restrictions (an exception list).</skos:definition>
      <rdfs:domain rdf:resource="&fibo-sec-sec-rst;BlueSkyRegulation"/>
      <rdfs:range rdf:resource="&fibo-fnd-plcx-gpli;USState"/>
   </owl:ObjectProperty>

   <owl:ObjectProperty rdf:about="&fibo-sec-sec-rst;hasRestrictions">
      <rdfs:label>has restrictions</rdfs:label>
      <rdfs:subPropertyOf rdf:resource="&fibo-sec-sec-rst;hasRestrictions.1"/>
      <rdfs:domain rdf:resource="&fibo-sec-sec-sec;ExchangeTradedSecurity"/>
      <rdfs:range rdf:resource="&fibo-sec-sec-rst;InvestmentRestriction"/>
   </owl:ObjectProperty>

   <owl:ObjectProperty rdf:about="&fibo-sec-sec-rst;hasRestrictions.1">
      <rdfs:label>has restrictions</rdfs:label>
      <skos:definition>Restrictions applicable to the Security</skos:definition>
      <rdfs:domain rdf:resource="&fibo-sec-sec-fi;FinancialInstrument"/>
      <rdfs:range rdf:resource="&fibo-sec-sec-rst;InvestmentRestriction"/>
   </owl:ObjectProperty>

   <owl:ObjectProperty rdf:about="&fibo-sec-sec-rst;restricts">
      <rdfs:label>restricts</rdfs:label>
      <rdfs:subPropertyOf rdf:resource="&fibo-fnd-lawx-rst;restricts.1"/>
      <rdfs:domain rdf:resource="&fibo-sec-sec-rst;InvestmentRestriction"/>
      <rdfs:range rdf:resource="&fibo-sec-sec-fi;FinancialInstrument"/>
   </owl:ObjectProperty>

   <owl:ObjectProperty rdf:about="&fibo-sec-sec-rst;investorDomicileRestrictionType">
      <rdfs:label>investor domicile restriction type</rdfs:label>
      <skos:definition>Specifies whether the restriction to be applied is relevant for citizen, resident, country. This property must be applied for this type of Restriction (it is optional in the parent class).</skos:definition>
      <rdfs:domain rdf:resource="&fibo-sec-sec-rst;InvestorsDomicileRestriction"/>
      <rdfs:range rdf:resource="&fibo-sec-sec-rst;InvestorDomicileType"/>
   </owl:ObjectProperty>

   <owl:ObjectProperty rdf:about="&fibo-sec-sec-rst;holdingPeriod">
      <rdfs:label>holding period</rdfs:label>
      <skos:definition>Period during which only Accredited Investors may hold the Security.</skos:definition>
      <rdfs:domain rdf:resource="&fibo-sec-sec-rst;QualifiedInvestorsRestriction"/>
      <rdfs:range rdf:resource="&fibo-fnd-tim-tim;Duration"/>
   </owl:ObjectProperty>

   <owl:ObjectProperty rdf:about="&fibo-sec-sec-rst;investorType">
      <rdfs:label>investor type</rdfs:label>
      <skos:definition>Type of investor that is allowed to hold the security. This property must be applied for this type of Restriction (it is optional in the parent class).</skos:definition>
      <rdfs:domain rdf:resource="&fibo-sec-sec-rst;QualifiedInvestorsRestriction"/>
      <rdfs:range rdf:resource="&fibo-sec-sec-rst;InvestorType"/>
   </owl:ObjectProperty>

   <owl:ObjectProperty rdf:about="&fibo-sec-sec-rst;appliesTo">
      <rdfs:label>applies to</rdfs:label>
      <rdfs:domain rdf:resource="&fibo-sec-sec-rst;SecurityRegistrationRequirement"/>
      <rdfs:range rdf:resource="&fibo-sec-sec-sec;Security"/>
      <owl:inverseOf rdf:resource="&fibo-sec-sec-rst;hasRegistrationRequirement"/>
   </owl:ObjectProperty>

   <owl:ObjectProperty rdf:about="&fibo-sec-sec-rst;holdingPeriod.1">
      <rdfs:label>holding period</rdfs:label>
      <skos:definition>Two-year holding period requirement on privately placed securities to permit qualified institutional buyers to trade these positions among themselves.</skos:definition>
      <rdfs:domain rdf:resource="&fibo-sec-sec-rst;Restriction144A"/>
      <rdfs:range rdf:resource="&fibo-fnd-tim-tim;Duration"/>
   </owl:ObjectProperty>

   <owl:ObjectProperty rdf:about="&fibo-sec-sec-rst;investorType.1">
      <rdfs:label>investor type</rdfs:label>
      <skos:definition>Investor type is restricted to Professional Investors for the stipulated time period.</skos:definition>
      <rdfs:domain rdf:resource="&fibo-sec-sec-rst;Restriction144A"/>
      <rdfs:range rdf:resource="&fibo-sec-sec-rst;InvestorType"/>
   </owl:ObjectProperty>

   <owl:ObjectProperty rdf:about="&fibo-sec-sec-rst;contractuallyDefinesRestrictions">
      <rdfs:label>contractually defines restrictions</rdfs:label>
      <rdfs:subPropertyOf rdf:resource="&fibo-fnd-lawx-rst;defines"/>
      <rdfs:domain rdf:resource="&fibo-sec-sec-sec;Security"/>
      <rdfs:range rdf:resource="&fibo-sec-sec-rst;SecurityContractualRestriction"/>
   </owl:ObjectProperty>

   <owl:ObjectProperty rdf:about="&fibo-sec-sec-rst;hasRestriction">
      <rdfs:label>has restriction</rdfs:label>
      <rdfs:subPropertyOf rdf:resource="&fibo-sec-sec-rst;hasRestrictions.1"/>
      <rdfs:domain rdf:resource="&fibo-sec-sec-sec;Security"/>
      <rdfs:range rdf:resource="&fibo-sec-sec-rst;InvestmentRestriction"/>
   </owl:ObjectProperty>

   <owl:ObjectProperty rdf:about="&fibo-sec-sec-rst;hasRegistrationRequirement">
      <rdfs:label>has registration requirement</rdfs:label>
      <rdfs:domain rdf:resource="&fibo-sec-sec-sec;Security"/>
      <rdfs:range rdf:resource="&fibo-sec-sec-rst;SecurityRegistrationRequirement"/>
   </owl:ObjectProperty>

   <owl:ObjectProperty rdf:about="&fibo-sec-sec-rst;holderRestrictions">
      <rdfs:label>holder restrictions</rdfs:label>
      <rdfs:subPropertyOf rdf:resource="&fibo-sec-sec-rst;hasRestrictions.1"/>
      <rdfs:domain rdf:resource="&fibo-sec-sec-sec;Security"/>
      <rdfs:range rdf:resource="&fibo-sec-sec-rst;LegalHoldingRestriction"/>
   </owl:ObjectProperty>

   <owl:ObjectProperty rdf:about="&fibo-sec-sec-rst;investorDomicileRestrictionType.1">
      <rdfs:label>investor domicile restriction type</rdfs:label>
      <skos:definition>Specifies whether the restriction to be applied is relevant for citizen, resident, country.</skos:definition>
      <rdfs:domain rdf:resource="&fibo-sec-sec-rst;LegalHoldingRestriction"/>
      <rdfs:range rdf:resource="&fibo-sec-sec-rst;InvestorDomicileType"/>
   </owl:ObjectProperty>

   <owl:ObjectProperty rdf:about="&fibo-sec-sec-rst;investorType.2">
      <rdfs:label>investor type</rdfs:label>
      <skos:definition>Type of investor that is allowed to hold the security.</skos:definition>
      <rdfs:domain rdf:resource="&fibo-sec-sec-rst;LegalHoldingRestriction"/>
      <rdfs:range rdf:resource="&fibo-sec-sec-rst;InvestorType"/>
   </owl:ObjectProperty>

   <owl:ObjectProperty rdf:about="&fibo-sec-sec-rst;appliesIn">
      <rdfs:label>applies in</rdfs:label>
      <rdfs:subPropertyOf rdf:resource="&fibo-fnd-lawx-rst;appliesIn"/>
      <rdfs:domain rdf:resource="&fibo-sec-sec-rst;InvestmentRestriction"/>
      <rdfs:range rdf:resource="&fibo-fnd-law-jur;Jurisdiction"/>
   </owl:ObjectProperty>

   <owl:ObjectProperty rdf:about="&fibo-sec-sec-rst;definedIn">
      <rdfs:label>defined in</rdfs:label>
      <rdfs:subPropertyOf rdf:resource="&fibo-bp-reg-reg;definedIn"/>
      <rdfs:domain rdf:resource="&fibo-sec-sec-rst;InvestmentRegulatoryRequirement"/>
      <rdfs:range rdf:resource="&fibo-sec-sec-rst;InvestmentRegulatoryLaw"/>
   </owl:ObjectProperty>

   <owl:ObjectProperty rdf:about="&fibo-sec-sec-rst;effectivePeriod">
      <rdfs:label>effective period</rdfs:label>
      <skos:definition>Period during which the restriction applies.</skos:definition>
      <rdfs:domain rdf:resource="&fibo-sec-sec-rst;InvestmentRestriction"/>
      <rdfs:range rdf:resource="&fibo-fnd-tim-tim;DatePeriod"/>
   </owl:ObjectProperty>

   <owl:ObjectProperty rdf:about="&fibo-sec-sec-rst;definedIn.1">
      <rdfs:label>defined in</rdfs:label>
      <rdfs:subPropertyOf rdf:resource="&fibo-fnd-lawx-rst;definedIn.1"/>
      <rdfs:domain rdf:resource="&fibo-sec-sec-rst;InvestmentRestriction"/>
      <rdfs:range rdf:resource="&fibo-sec-sec-rst;InvestmentRegulatoryLaw"/>
   </owl:ObjectProperty>


  <!--
    ///////////////////////////////////////////////////////////////////////////////////////
    //
    // Data Properties
    //
    ///////////////////////////////////////////////////////////////////////////////////////
    -->


<owl:DatatypeProperty rdf:about="&fibo-sec-sec-rst;inclusive">
      <rdfs:label>inclusive</rdfs:label>
      <skos:definition>The Blue Sky Regulatory Requirement is framed in terms of the States NOT covered by the Regulation.</skos:definition>
      <rdfs:range rdf:resource="&fibo-fnd-utl-bt;yesOrNo"/>
   </owl:DatatypeProperty>

   <owl:DatatypeProperty rdf:about="&fibo-sec-sec-rst;inclusive.1">
      <rdfs:label>inclusive</rdfs:label>
      <skos:definition>Note: Regulation S is an exclusive restriction for Investor Domicile Type (Type = Resident, Inclusive = no), but Exclusive for Investor Type (Type = Professional, Inclusive = yes). Remodel this during review.</skos:definition>
      <rdfs:range rdf:resource="&fibo-fnd-utl-bt;yesOrNo"/>
   </owl:DatatypeProperty>

   <owl:DatatypeProperty rdf:about="&fibo-sec-sec-rst;inclusive.2">
      <rdfs:label>inclusive</rdfs:label>
      <skos:definition>The restriction includes the party mentioned in the investor restriction type.</skos:definition>
      <rdfs:range rdf:resource="&fibo-fnd-utl-bt;yesOrNo"/>
   </owl:DatatypeProperty>

   <owl:DatatypeProperty rdf:about="&fibo-sec-sec-rst;inclusive.3">
      <rdfs:label>inclusive</rdfs:label>
      <skos:definition>Whether the Restriction is defined inclusively (the stated terms put something within the Restriction), or Exclusively (the stated terms put something outside the reach or remit of the Restriction). Yes = Inclusive.</skos:definition>
      <rdfs:range rdf:resource="&fibo-fnd-utl-bt;yesOrNo"/>
   </owl:DatatypeProperty>

   <owl:DatatypeProperty rdf:about="&fibo-sec-sec-rst;inclusive.4">
      <rdfs:label>inclusive</rdfs:label>
      <skos:definition>Whether the restriction includes or excludes the party mentioned in the investor restriction type.</skos:definition>
      <rdfs:range rdf:resource="&fibo-fnd-utl-bt;yesOrNo"/>
   </owl:DatatypeProperty>

   <owl:DatatypeProperty rdf:about="&fibo-sec-sec-rst;description">
      <rdfs:label>description</rdfs:label>
      <skos:definition>Free text description of the restriction.</skos:definition>
      <rdfs:range rdf:resource="&fibo-fnd-utl-bt;text"/>
   </owl:DatatypeProperty>

   <owl:DatatypeProperty rdf:about="&fibo-sec-sec-rst;rate">
      <rdfs:label>rate</rdfs:label>
      <skos:definition>Rate used for the calculation of the restriction.</skos:definition>
      <rdfs:range rdf:resource="&fibo-fnd-utl-bt;percentage"/>
   </owl:DatatypeProperty>


  <!--
    ///////////////////////////////////////////////////////////////////////////////////////
    //
    // Annotation Properties
    //
    ///////////////////////////////////////////////////////////////////////////////////////
    -->



  <!--
    ///////////////////////////////////////////////////////////////////////////////////////
    //
    // Classes
    //
    ///////////////////////////////////////////////////////////////////////////////////////
    -->


<owl:Class rdf:about="&fibo-sec-sec-rst;BlueSkyRegulation">
      <rdfs:label>blue sky regulation</rdfs:label>
      <skos:definition>State regulations designed to protect investors against securities fraud by requiring sellers of new issues to register their offerings and provide financial details. This allows investors to base their judgments on trustworthy data.</skos:definition>
      <rdfs:subClassOf rdf:resource="&fibo-sec-sec-rst;SecurityRegistrationRequirement"/>
   </owl:Class>

   <owl:Class rdf:about="&fibo-sec-sec-rst;InvestorsDomicileRestriction">
      <rdfs:label>investors domicile restriction</rdfs:label>
      <skos:definition>Restriction defining where holders of a security may be domiciled.</skos:definition>
      <rdfs:subClassOf rdf:resource="&fibo-sec-sec-rst;LegalHoldingRestriction"/>
   </owl:Class>

   <owl:Class rdf:about="&fibo-sec-sec-rst;QualifiedInvestorsRestriction">
      <rdfs:label>qualified investors restriction</rdfs:label>
      <skos:definition>A Restriction in which only qualified investors may hold the Security, optionally for a definede Holding Period (if this is not defined then the period is indefinite).</skos:definition>
   </owl:Class>

   <owl:Class rdf:about="&fibo-sec-sec-rst;RegulationS">
      <rdfs:label>regulation s</rdfs:label>
      <skos:definition>Regulation S is the exemption through which corporations can issue unregistered securities to qualified foreign investors and foreign institutions</skos:definition>
      <rdfs:subClassOf rdf:resource="&fibo-sec-sec-rst;QualifiedInvestorsRestriction"/>
      <rdfs:subClassOf rdf:resource="&fibo-sec-sec-rst;InvestorsDomicileRestriction"/>
   </owl:Class>

   <owl:Class rdf:about="&fibo-sec-sec-rst;Restriction144A">
      <rdfs:label>restriction 144 a</rdfs:label>
      <skos:definition>A Securities & Exchange Commission rule modifying a two-year holding period requirement on privately placed securities to permit qualified institutional buyers to trade these positions among themselves.</skos:definition>
   </owl:Class>

   <owl:Class rdf:about="&fibo-sec-sec-rst;SecurityContractualRestriction">
      <rdfs:label>security contractual restriction</rdfs:label>
      <skos:definition>Contractual terms setting out restrictions on either the holder or the issuer of the security.</skos:definition>
      <rdfs:subClassOf rdf:resource="&fibo-fnd-lawx-rst;ContractualRestriction"/>
   </owl:Class>

   <owl:Class rdf:about="&fibo-sec-sec-rst;SecurityRegistrationRequirement">
      <rdfs:label>security registration requirement</rdfs:label>
      <skos:definition>A Requirement for Registraton of a Security within some Country, Jurisdiction or Federal Province.</skos:definition>
      <rdfs:subClassOf rdf:resource="&fibo-sec-sec-rst;InvestmentRegulatoryRequirement"/>
   </owl:Class>

   <owl:Class rdf:about="&fibo-sec-sec-rst;LegalHoldingRestriction">
      <rdfs:label>legal holding restriction</rdfs:label>
      <skos:definition>Restrictions applicable to holding of the security.</skos:definition>
      <rdfs:subClassOf rdf:resource="&fibo-sec-sec-rst;InvestmentRestriction"/>
   </owl:Class>

   <owl:Class rdf:about="&fibo-sec-sec-rst;TradingRestriction">
      <rdfs:label>trading restriction</rdfs:label>
   </owl:Class>

   <owl:Class rdf:about="&fibo-sec-sec-rst;InvestmentRegulatoryLaw">
      <rdfs:label>investment regulatory law</rdfs:label>
      <skos:definition>A body of law dealing with investment regulation.</skos:definition>
      <rdfs:subClassOf rdf:resource="&fibo-fnd-law-jur;StatuteLaw"/>
   </owl:Class>

   <owl:Class rdf:about="&fibo-sec-sec-rst;InvestmentRegulatoryRequirement">
      <rdfs:label>investment regulatory requirement</rdfs:label>
      <skos:definition>A requirement laid down in law for investment regulation.</skos:definition>
      <rdfs:subClassOf rdf:resource="&fibo-fnd-lawx-rst;RegulatoryRequirement"/>
   </owl:Class>

   <owl:Class rdf:about="&fibo-sec-sec-rst;InvestmentRestriction">
      <rdfs:label>investment restriction</rdfs:label>
      <skos:definition>Restrictions applicable to a financial instrument as provided for in a body of Law.</skos:definition>
      <rdfs:subClassOf rdf:resource="&fibo-fnd-lawx-rst;LegalRestriction"/>
   </owl:Class>


  <!--
    ///////////////////////////////////////////////////////////////////////////////////////
    //
    // Individuals
    //
    ///////////////////////////////////////////////////////////////////////////////////////
    -->


</rdf:RDF>