<?xml version="1.0" encoding="UTF-8"?>
<!DOCTYPE rdf:RDF [
	<!ENTITY dct "http://purl.org/dc/terms/">
	<!ENTITY fibo-fnd-agr-ctr "https://spec.edmcouncil.org/fibo/FND/Agreements/Contracts/">
	<!ENTITY fibo-fnd-dt-fd "https://spec.edmcouncil.org/fibo/FND/DatesAndTimes/FinancialDates/">
	<!ENTITY fibo-fnd-utl-av "https://spec.edmcouncil.org/fibo/FND/Utilities/AnnotationVocabulary/">
	<!ENTITY fibo-fnd-utlx-val "https://spec.edmcouncil.org/fibo/FND/UtilitiesExt/Values/">
	<!ENTITY fibo-md-dbtx-int "https://spec.edmcouncil.org/fibo/MD/DebtTemporal/DebtInterestAmounts/">
	<!ENTITY fibo-sec-dbt-bo-bo "https://spec.edmcouncil.org/fibo/SEC/Debt/Bonds/BondsCommon/">
	<!ENTITY fibo-sec-dbt-bo-cft "https://spec.edmcouncil.org/fibo/SEC/Debt/Bonds/BondsCashflowTerms/">
	<!ENTITY fibo-sec-dbt-bo-cfv "https://spec.edmcouncil.org/fibo/SEC/Debt/Bonds/BondsCashflowVariants/">
	<!ENTITY fibo-sec-dbt-bo-iss "https://spec.edmcouncil.org/fibo/SEC/Debt/Bonds/BondsIssuerVariants/">
	<!ENTITY fibo-sec-dbt-bo-li "https://spec.edmcouncil.org/fibo/SEC/Debt/Bonds/BondsListings/">
	<!ENTITY fibo-sec-dbt-dbt-cft "https://spec.edmcouncil.org/fibo/SEC/Debt/DebtFoundations/DebtCashflowTerms/">
	<!ENTITY fibo-sec-dbt-dbti "https://spec.edmcouncil.org/fibo/SEC/Debt/DebtInstruments/">
	<!ENTITY fibo-sec-eq-eq "https://spec.edmcouncil.org/fibo/SEC/Equities/EquityInstruments/">
	<!ENTITY fibo-sec-sec-iss "https://spec.edmcouncil.org/fibo/SEC/Securities/SecuritiesIssuance/">
	<!ENTITY fibo-sec-sec-lst "https://spec.edmcouncil.org/fibo/SEC/Securities/SecuritiesListings/">
	<!ENTITY owl "http://www.w3.org/2002/07/owl#">
	<!ENTITY rdf "http://www.w3.org/1999/02/22-rdf-syntax-ns#">
	<!ENTITY rdfs "http://www.w3.org/2000/01/rdf-schema#">
	<!ENTITY skos "http://www.w3.org/2004/02/skos/core#">
	<!ENTITY terms "http://purl.org/dc/terms/">
	<!ENTITY xsd "http://www.w3.org/2001/XMLSchema#">
]>
<rdf:RDF xml:base="https://spec.edmcouncil.org/fibo/SEC/Debt/Bonds/BondsCommon/"
	xmlns:dct="http://purl.org/dc/terms/"
	xmlns:fibo-fnd-agr-ctr="https://spec.edmcouncil.org/fibo/FND/Agreements/Contracts/"
	xmlns:fibo-fnd-dt-fd="https://spec.edmcouncil.org/fibo/FND/DatesAndTimes/FinancialDates/"
	xmlns:fibo-fnd-utl-av="https://spec.edmcouncil.org/fibo/FND/Utilities/AnnotationVocabulary/"
	xmlns:fibo-fnd-utlx-val="https://spec.edmcouncil.org/fibo/FND/UtilitiesExt/Values/"
	xmlns:fibo-md-dbtx-int="https://spec.edmcouncil.org/fibo/MD/DebtTemporal/DebtInterestAmounts/"
	xmlns:fibo-sec-dbt-bo-bo="https://spec.edmcouncil.org/fibo/SEC/Debt/Bonds/BondsCommon/"
	xmlns:fibo-sec-dbt-bo-cft="https://spec.edmcouncil.org/fibo/SEC/Debt/Bonds/BondsCashflowTerms/"
	xmlns:fibo-sec-dbt-bo-cfv="https://spec.edmcouncil.org/fibo/SEC/Debt/Bonds/BondsCashflowVariants/"
	xmlns:fibo-sec-dbt-bo-iss="https://spec.edmcouncil.org/fibo/SEC/Debt/Bonds/BondsIssuerVariants/"
	xmlns:fibo-sec-dbt-bo-li="https://spec.edmcouncil.org/fibo/SEC/Debt/Bonds/BondsListings/"
	xmlns:fibo-sec-dbt-dbt-cft="https://spec.edmcouncil.org/fibo/SEC/Debt/DebtFoundations/DebtCashflowTerms/"
	xmlns:fibo-sec-dbt-dbti="https://spec.edmcouncil.org/fibo/SEC/Debt/DebtInstruments/"
	xmlns:fibo-sec-eq-eq="https://spec.edmcouncil.org/fibo/SEC/Equities/EquityInstruments/"
	xmlns:fibo-sec-sec-iss="https://spec.edmcouncil.org/fibo/SEC/Securities/SecuritiesIssuance/"
	xmlns:fibo-sec-sec-lst="https://spec.edmcouncil.org/fibo/SEC/Securities/SecuritiesListings/"
	xmlns:owl="http://www.w3.org/2002/07/owl#"
	xmlns:rdf="http://www.w3.org/1999/02/22-rdf-syntax-ns#"
	xmlns:rdfs="http://www.w3.org/2000/01/rdf-schema#"
	xmlns:skos="http://www.w3.org/2004/02/skos/core#"
	xmlns:terms="http://purl.org/dc/terms/"
	xmlns:xsd="http://www.w3.org/2001/XMLSchema#">
	
	<owl:Ontology rdf:about="https://spec.edmcouncil.org/fibo/SEC/Debt/Bonds/BondsCommon/">
		<rdfs:label xml:lang="en">BondsCommon</rdfs:label>
		<terms:abstract>This ontology defines the basic concept of a bond and a number of bond variants including convertible and callable bonds. Medium term notes (MTNs) and debentures are also defined.</terms:abstract>
		<owl:imports rdf:resource="http://www.w3.org/2004/02/skos/core"/>
		<owl:imports rdf:resource="https://spec.edmcouncil.org/fibo/DER/RightsInstruments/RightsAndWarrants/"/>
		<owl:imports rdf:resource="https://spec.edmcouncil.org/fibo/FBC/DebtAndEquities/Debt/"/>
		<owl:imports rdf:resource="https://spec.edmcouncil.org/fibo/FBC/FinancialInstruments/FinancialInstruments/"/>
		<owl:imports rdf:resource="https://spec.edmcouncil.org/fibo/FND/Agreements/Contracts/"/>
		<owl:imports rdf:resource="https://spec.edmcouncil.org/fibo/FND/DatesAndTimes/FinancialDates/"/>
		<owl:imports rdf:resource="https://spec.edmcouncil.org/fibo/FND/Parties/Parties/"/>
		<owl:imports rdf:resource="https://spec.edmcouncil.org/fibo/FND/Relations/Relations/"/>
		<owl:imports rdf:resource="https://spec.edmcouncil.org/fibo/FND/Utilities/AnnotationVocabulary/"/>
		<owl:imports rdf:resource="https://spec.edmcouncil.org/fibo/FND/UtilitiesExt/Values/"/>
		<owl:imports rdf:resource="https://spec.edmcouncil.org/fibo/IND/EconomicIndicators/EconomicIndicators/"/>
		<owl:imports rdf:resource="https://spec.edmcouncil.org/fibo/MD/DebtTemporal/DebtInterestAmounts/"/>
		<owl:imports rdf:resource="https://spec.edmcouncil.org/fibo/SEC/Debt/Bonds/BondsCashflowTerms/"/>
		<owl:imports rdf:resource="https://spec.edmcouncil.org/fibo/SEC/Debt/Bonds/BondsCashflowVariants/"/>
		<owl:imports rdf:resource="https://spec.edmcouncil.org/fibo/SEC/Debt/Bonds/BondsIssuerVariants/"/>
		<owl:imports rdf:resource="https://spec.edmcouncil.org/fibo/SEC/Debt/Bonds/BondsListings/"/>
		<owl:imports rdf:resource="https://spec.edmcouncil.org/fibo/SEC/Debt/DebtFoundations/DebtCashflowTerms/"/>
		<owl:imports rdf:resource="https://spec.edmcouncil.org/fibo/SEC/Debt/DebtFoundations/DebtIssuanceTerms/"/>
		<owl:imports rdf:resource="https://spec.edmcouncil.org/fibo/SEC/Debt/DebtInstruments/"/>
		<owl:imports rdf:resource="https://spec.edmcouncil.org/fibo/SEC/Equities/EquityInstruments/"/>
		<owl:imports rdf:resource="https://spec.edmcouncil.org/fibo/SEC/Securities/SecuritiesIssuance/"/>
		<owl:imports rdf:resource="https://spec.edmcouncil.org/fibo/SEC/Securities/SecuritiesListings/"/>
		<owl:versionIRI rdf:resource="https://spec.edmcouncil.org/fibo/SEC/Debt/Bonds/BondsCommon/"/>
		<fibo-fnd-utl-av:hasMaturityLevel rdf:resource="&fibo-fnd-utl-av;Provisional"/>
	</owl:Ontology>
	
	<owl:Class rdf:about="&fibo-sec-dbt-bo-bo;Bond">
		<rdfs:subClassOf rdf:resource="&fibo-sec-dbt-dbti;TradableDebtInstrument"/>
		<rdfs:subClassOf>
			<owl:Restriction>
				<owl:onProperty rdf:resource="&fibo-md-dbtx-int;bondHasCoupon"/>
				<owl:someValuesFrom rdf:resource="&fibo-md-dbtx-int;BondCoupon"/>
			</owl:Restriction>
		</rdfs:subClassOf>
		<rdfs:subClassOf>
			<owl:Restriction>
				<owl:onProperty rdf:resource="&fibo-sec-dbt-bo-cft;hasCouponStructureTerms"/>
				<owl:someValuesFrom rdf:resource="&fibo-sec-dbt-bo-cft;BondCouponStructureType"/>
			</owl:Restriction>
		</rdfs:subClassOf>
		<rdfs:subClassOf>
			<owl:Restriction>
				<owl:onProperty rdf:resource="&fibo-sec-dbt-bo-bo;isConvertible"/>
				<owl:someValuesFrom rdf:resource="&xsd;boolean"/>
			</owl:Restriction>
		</rdfs:subClassOf>
		<rdfs:subClassOf>
			<owl:Restriction>
				<owl:onProperty rdf:resource="&fibo-sec-dbt-dbti;hasRepaymentTerms"/>
				<owl:someValuesFrom rdf:resource="&fibo-sec-dbt-bo-cft;BondPrincipalRepaymentTermsSet"/>
			</owl:Restriction>
		</rdfs:subClassOf>
		<rdfs:subClassOf>
			<owl:Restriction>
				<owl:onProperty rdf:resource="&fibo-sec-dbt-dbti;isCallable"/>
				<owl:someValuesFrom rdf:resource="&xsd;boolean"/>
			</owl:Restriction>
		</rdfs:subClassOf>
		<rdfs:label xml:lang="en">bond</rdfs:label>
		<skos:definition xml:lang="en">A debt security, in which the authorized issuer owes the holders a debt and, depending on the terms of the bond, is obliged to pay interest (the coupon) and/or to repay the principal at a later date, termed maturity. It is a formal contract to repay borrowed money with interest at fixed intervals.</skos:definition>
		<skos:editorialNote xml:lang="en">30 Sept 2010: Original definition updated by MBS PoC project and agreed. Tidies the language in the original Wikipedia-drived definition. Consensus attained.</skos:editorialNote>
	</owl:Class>
	
	<owl:Class rdf:about="&fibo-sec-dbt-bo-bo;BondWithPartialCall">
		<rdfs:subClassOf rdf:resource="&fibo-sec-dbt-bo-bo;CallableBond"/>
		<rdfs:subClassOf>
			<owl:Restriction>
				<owl:onProperty rdf:resource="&fibo-sec-dbt-dbti;hasCallFeature"/>
				<owl:someValuesFrom rdf:resource="&fibo-sec-dbt-bo-cft;PartialCallFeature"/>
			</owl:Restriction>
		</rdfs:subClassOf>
		<rdfs:label xml:lang="en">bond with partial call</rdfs:label>
		<skos:definition xml:lang="en">A bond with a feature whereby the issue can be partially called for amounts that are at the discretion of the issuer.</skos:definition>
	</owl:Class>
	
	<owl:Class rdf:about="&fibo-sec-dbt-bo-bo;BondWithWarrant">
		<rdfs:subClassOf rdf:resource="&fibo-sec-dbt-bo-bo;Bond"/>
		<rdfs:label xml:lang="en">bond with warrant</rdfs:label>
		<skos:definition xml:lang="en">A bond issue where the issue includes a Warrant attached. This need not be any specific type of bond.</skos:definition>
		<skos:editorialNote xml:lang="en">This is NOT a kind of Bond Contract but a kind of Issue Offer, and is modeled as such, in the Issuance Terms section of the model. This class of contract is retained in the model for now in order to provide traceability with the CFI term for &quot;Bond With Warrant&quot; only.</skos:editorialNote>
	</owl:Class>
	
	<owl:Class rdf:about="&fibo-sec-dbt-bo-bo;CallableBond">
		<rdfs:subClassOf rdf:resource="&fibo-sec-dbt-bo-bo;Bond"/>
		<rdfs:subClassOf>
			<owl:Restriction>
				<owl:onProperty rdf:resource="&fibo-sec-dbt-dbti;hasCallFeature"/>
				<owl:someValuesFrom rdf:resource="&fibo-sec-dbt-bo-cft;BondCallTermsSet"/>
			</owl:Restriction>
		</rdfs:subClassOf>
		<rdfs:label xml:lang="en">callable bond</rdfs:label>
		<terms:description xml:lang="en">A bond with call provisions, or callable bond, is a bond that can be redeemed by the issuer prior to its maturity.</terms:description>
		<fibo-fnd-utl-av:definitionOrigin xml:lang="en">Investopedia</fibo-fnd-utl-av:definitionOrigin>
	</owl:Class>
	
	<owl:Class rdf:about="&fibo-sec-dbt-bo-bo;CallableConvertibleBond">
		<rdfs:subClassOf rdf:resource="&fibo-sec-dbt-bo-bo;CallableBond"/>
		<rdfs:subClassOf rdf:resource="&fibo-sec-dbt-bo-bo;ConvertibleBond"/>
		<rdfs:subClassOf>
			<owl:Restriction>
				<owl:onProperty rdf:resource="&fibo-sec-dbt-dbti;isCallable"/>
				<owl:someValuesFrom rdf:resource="&xsd;boolean"/>
			</owl:Restriction>
		</rdfs:subClassOf>
		<rdfs:label xml:lang="en">callable convertible bond</rdfs:label>
		<skos:definition xml:lang="en">A Convertible Bond which is also callable.</skos:definition>
	</owl:Class>
	
	<owl:Class rdf:about="&fibo-sec-dbt-bo-bo;ConvertibleBond">
		<rdfs:subClassOf rdf:resource="&fibo-sec-dbt-bo-bo;Bond"/>
		<rdfs:subClassOf>
			<owl:Restriction>
				<owl:onProperty rdf:resource="&fibo-fnd-agr-ctr;hasContractualElement"/>
				<owl:someValuesFrom rdf:resource="&fibo-sec-dbt-bo-bo;DebtConversionTerms"/>
			</owl:Restriction>
		</rdfs:subClassOf>
		<rdfs:subClassOf>
			<owl:Restriction>
				<owl:onProperty rdf:resource="&fibo-sec-dbt-bo-bo;convertibleInto"/>
				<owl:someValuesFrom rdf:resource="&fibo-sec-eq-eq;PubliclyTradedShare"/>
			</owl:Restriction>
		</rdfs:subClassOf>
		<rdfs:subClassOf>
			<owl:Restriction>
				<owl:onProperty rdf:resource="&fibo-sec-dbt-bo-bo;isConvertible"/>
				<owl:someValuesFrom rdf:resource="&xsd;boolean"/>
			</owl:Restriction>
		</rdfs:subClassOf>
		<rdfs:label xml:lang="en">convertible bond</rdfs:label>
		<skos:definition xml:lang="en">A Bond instrument which on maturity converts into an Equity instrument.</skos:definition>
		<skos:editorialNote xml:lang="en">There are different types based on the available exercise windows and facts thereof. Notes from CAE review on 7 July 2011 1. Convertible - meaning a convertible Bond whi ch converts into an Equity later in its life 2. Contingent Conversion (of what? - of a Debt. So it&apos;s a kind of Convertible) - if the share price reaches a particular threshold on a particular time window = COCO. - this is a debt instrument. you get the share when it reaches that price threshold. There are time windows (like traditional options instruments - i.e. Bermudan?) - is it mandatory to take a share it&apos;s mandatory - like a digital options which are also not really optional . The distinction is the time window.</skos:editorialNote>
	</owl:Class>
	
	<owl:Class rdf:about="&fibo-sec-dbt-bo-bo;Debenture">
		<rdfs:subClassOf rdf:resource="&fibo-sec-dbt-bo-bo;Bond"/>
		<rdfs:subClassOf>
			<owl:Restriction>
				<owl:onProperty rdf:resource="&fibo-sec-dbt-bo-bo;securitizationConditions.1"/>
				<owl:onClass rdf:resource="&fibo-sec-dbt-bo-bo;DebentureSecuritizationConditions"/>
				<owl:maxQualifiedCardinality rdf:datatype="&xsd;nonNegativeInteger">1</owl:maxQualifiedCardinality>
			</owl:Restriction>
		</rdfs:subClassOf>
		<rdfs:label xml:lang="en">debenture</rdfs:label>
		<skos:definition xml:lang="en">A type of debt instrument that is not secured by physical asset or collateral. Debentures are backed only by the general creditworthiness and reputation of the issuer. Both corporations and governments frequently issue this type of bond in order to secure capital. Like other types of bonds, debentures are documented in an indenture.</skos:definition>
		<fibo-fnd-utl-av:explanatoryNote xml:lang="en">From Wikipedia: In law, a debenture is a document which either creates a debt or acknowledges it. It is a medium to long-term borrowing facility created by a company. Where repayment is secured by a charge over land, the document is called a &apos;mortgage&apos;. Where repayment is secured by a charge other assets of the company, the document is called a &apos;debenture&apos;. Where no security is involved, the document is called a note or &apos;unsecured deposit note&apos;. There are two types of debentures: 1. Convertible Debentures, which are convertible bonds or bonds that can be converted into equity shares of the issuing company after a predetermined period of time. &quot;Convertibility&quot; is a feature that corporations may add to the bonds they issue in order to make them more attractive to buyers. In other words, it is a special feature that a corporate bond may carry. As a result of the advantage a buyer gets from the ability to convert, convertible bonds typically have lower interest rates than non-convertible corporate bonds. 2. Non-Convertible Debentures, which are simply regular debentures, cannot be converted into equity shares of the liable company. They are debentures without the convertibility feature attached to them. As a result, they usually carry higher interest rates than their convertible counterparts.</fibo-fnd-utl-av:explanatoryNote>
	</owl:Class>
	
	<owl:Class rdf:about="&fibo-sec-dbt-bo-bo;DebentureSecuritizationConditions">
		<rdfs:subClassOf rdf:resource="&fibo-fnd-agr-ctr;ContractualCommitment"/>
		<rdfs:label xml:lang="en">debenture securitization conditions</rdfs:label>
		<skos:definition xml:lang="en">Terms, if any, by which a Debenture is secured. This is a description of the properties by which it is secured, being those not otherwise pledged.</skos:definition>
		<skos:editorialNote xml:lang="en">From original model (whose?): A debenture is usually unsecured in the sense that there are no liens or pledges on specific assets. It is however, secured by all properties not otherwise pledged. From Wikipedia A debenture (also called a note) is an unsecured corporate bond or a corporate bond that does not have a certain line of income or piece of property or equipment to guarantee repayment of principal upon the bond&apos;s maturity. Debentures are long-term debt instrument used by large companies to obtain funds. Where securities are offered, loan stocks or bonds are termed &apos;debentures&apos; in the UK or &apos;mortgage bonds&apos; in the US. Summary: Therefore they are unsecured in the sense of not having a particular cash flow allocated to them, but they are therefore secured by some other asset.</skos:editorialNote>
	</owl:Class>
	
	<owl:Class rdf:about="&fibo-sec-dbt-bo-bo;DebtConversionTerms">
		<rdfs:subClassOf rdf:resource="&fibo-sec-dbt-dbti;TradableDebtInstrumentRedemptionProvision"/>
		<rdfs:subClassOf rdf:resource="&fibo-sec-sec-iss;ConversionTerms"/>
		<rdfs:subClassOf>
			<owl:Restriction>
				<owl:onProperty rdf:resource="&fibo-sec-sec-iss;specifiesConversionInto"/>
				<owl:someValuesFrom rdf:resource="&fibo-sec-eq-eq;PubliclyTradedShare"/>
			</owl:Restriction>
		</rdfs:subClassOf>
		<rdfs:label xml:lang="en">debt conversion terms</rdfs:label>
		<skos:definition xml:lang="en">Contractual specifications when a Convertible Bond can be converted to another security (usually of the same issuer).</skos:definition>
	</owl:Class>
	
	<owl:Class rdf:about="&fibo-sec-dbt-bo-bo;EquityLinkedBond">
		<rdfs:subClassOf rdf:resource="&fibo-sec-dbt-bo-cfv;VariableCouponBond"/>
		<rdfs:label xml:lang="en">equity linked bond</rdfs:label>
		<skos:definition xml:lang="en">A bond where the bond is based on the return on an equity over time i.e. the price and dividend payments i.e. the total return (similar to total return swaps).</skos:definition>
	</owl:Class>
	
	<owl:Class rdf:about="&fibo-sec-dbt-bo-bo;ListedBond">
		<rdfs:subClassOf rdf:resource="&fibo-sec-dbt-bo-bo;Bond"/>
		<rdfs:subClassOf rdf:resource="&fibo-sec-sec-lst;ExchangeTradedSecurity"/>
		<rdfs:subClassOf>
			<owl:Restriction>
				<owl:onProperty rdf:resource="&fibo-sec-sec-lst;isListedVia"/>
				<owl:someValuesFrom rdf:resource="&fibo-sec-dbt-bo-li;BondListing"/>
			</owl:Restriction>
		</rdfs:subClassOf>
		<rdfs:label xml:lang="en">listed bond</rdfs:label>
		<owl:disjointWith rdf:resource="&fibo-sec-dbt-bo-bo;UnlistedBond"/>
		<skos:definition xml:lang="en">A security that is a bond and is traded on an exchange.</skos:definition>
		<fibo-fnd-utl-av:explanatoryNote xml:lang="en">In principle this may be any type of bond other than an unlisted bond. Most exchange traded bonds are corporate bonds (but most corporate bonds are not exchange traded bonds). This is a common but not a necessary fact.</fibo-fnd-utl-av:explanatoryNote>
	</owl:Class>
	
	<owl:Class rdf:about="&fibo-sec-dbt-bo-bo;MediumTermNote">
		<rdfs:subClassOf rdf:resource="&fibo-sec-dbt-bo-bo;Bond"/>
		<rdfs:label xml:lang="en">medium term note</rdfs:label>
		<skos:definition xml:lang="en">A Medium Term Note is a Negotiable debt instrument offered under a program agreement through one or more dealers upon request of the Issuer. The Program defines the terms and conditions of the notes. An MTN issue is defined by the fact that the registration doesn&apos;t have a pre-defined maturity.</skos:definition>
		<fibo-fnd-utl-av:explanatoryNote xml:lang="en">MTNs have a maturity typically of 1 to 10 years. This may vary in different jurisductions. Bonds issued with a long maturity are not redefined as MTNs when their maturity reduces. MTN typically has a long last coupon payment. Some things are different from regular bonds, e.g.: You can register one with different maturities, issued in different groups (cf tranches). See also shelf registration (issuing bond before you file the paperwork with e.g. SEC - not the same). In this case it is registered but not issued all at one time. Flexible. Difference with bond issuance is that you have indenture that says what the maturity is, so every different maturity is a different bond.</fibo-fnd-utl-av:explanatoryNote>
	</owl:Class>
	
	<owl:Class rdf:about="&fibo-sec-dbt-bo-bo;UnlistedBond">
		<rdfs:subClassOf rdf:resource="&fibo-sec-dbt-bo-bo;Bond"/>
		<rdfs:label xml:lang="en">unlisted bond</rdfs:label>
		<terms:description xml:lang="en">A bond that is traded over the counter rather than via an exchange or other listing facility.</terms:description>
		<fibo-fnd-utl-av:synonym xml:lang="en">OTC Bond</fibo-fnd-utl-av:synonym>
	</owl:Class>
	
	<owl:ObjectProperty rdf:about="&fibo-sec-dbt-bo-bo;capitalizedInterest">
		<rdfs:label xml:lang="en">capitalized interest</rdfs:label>
		<rdfs:domain rdf:resource="&fibo-sec-dbt-bo-bo;Bond"/>
		<rdfs:range rdf:resource="&fibo-fnd-utlx-val;TrueFalseValue"/>
		<skos:definition xml:lang="en">Whether the interest amount is capitalised until maturity date or paid out at each interest payment date.</skos:definition>
	</owl:ObjectProperty>
	
	<owl:ObjectProperty rdf:about="&fibo-sec-dbt-bo-bo;convertibleInto">
		<rdfs:label xml:lang="en">convertible into</rdfs:label>
		<rdfs:domain rdf:resource="&fibo-sec-dbt-bo-bo;ConvertibleBond"/>
		<rdfs:range rdf:resource="&fibo-sec-eq-eq;PubliclyTradedShare"/>
	</owl:ObjectProperty>
	
	<owl:ObjectProperty rdf:about="&fibo-sec-dbt-bo-bo;extraordinaryRedemptionApplicable">
		<rdfs:label xml:lang="en">extraordinary redemption applicable</rdfs:label>
		<terms:description xml:lang="en">whether the security is subject to extraordinary redemption</terms:description>
		<rdfs:domain rdf:resource="&fibo-sec-dbt-bo-bo;Bond"/>
		<rdfs:range rdf:resource="&fibo-fnd-utlx-val;TrueFalseValue"/>
	</owl:ObjectProperty>
	
	<owl:ObjectProperty rdf:about="&fibo-sec-dbt-bo-bo;hasBondMaturityRegistrar">
		<rdfs:subPropertyOf rdf:resource="&fibo-fnd-agr-ctr;hasThirdParty"/>
		<rdfs:label xml:lang="en">has bond maturity registrar</rdfs:label>
		<rdfs:domain rdf:resource="&fibo-sec-dbt-bo-bo;Bond"/>
		<rdfs:range rdf:resource="&fibo-sec-dbt-bo-iss;BondMaturityRegistrar"/>
		<skos:definition xml:lang="en">The person or entity responsible for maintaining records on behalf of the issuer that identify the owners of a registered bond issue.</skos:definition>
	</owl:ObjectProperty>
	
	<owl:ObjectProperty rdf:about="&fibo-sec-dbt-bo-bo;hasConversionTerms">
		<rdfs:subPropertyOf rdf:resource="&fibo-fnd-agr-ctr;hasContractualElement"/>
		<rdfs:label xml:lang="en">has conversion terms</rdfs:label>
		<rdfs:domain rdf:resource="&fibo-sec-dbt-bo-bo;ConvertibleBond"/>
		<rdfs:range rdf:resource="&fibo-sec-dbt-bo-bo;DebtConversionTerms"/>
	</owl:ObjectProperty>
	
	<owl:ObjectProperty rdf:about="&fibo-sec-dbt-bo-bo;hasConvertibleDate">
		<rdfs:subPropertyOf rdf:resource="&fibo-fnd-dt-fd;hasDate"/>
		<rdfs:label xml:lang="en">has convertible date</rdfs:label>
		<rdfs:domain rdf:resource="&fibo-sec-dbt-bo-bo;DebtConversionTerms"/>
		<rdfs:range rdf:resource="&fibo-fnd-dt-fd;Date"/>
		<skos:definition>the date on which a bond can be converted into the specified equity security</skos:definition>
	</owl:ObjectProperty>
	
	<owl:ObjectProperty rdf:about="&fibo-sec-dbt-bo-bo;hasCouponInterestTerms">
		<rdfs:subPropertyOf rdf:resource="&fibo-sec-dbt-dbti;hasInterestPaymentTerms"/>
		<rdfs:label xml:lang="en">has coupon interest terms</rdfs:label>
		<rdfs:domain rdf:resource="&fibo-sec-dbt-bo-bo;Bond"/>
		<rdfs:range rdf:resource="&fibo-sec-dbt-bo-cft;BondCouponInterestTerms"/>
	</owl:ObjectProperty>
	
	<owl:DatatypeProperty rdf:about="&fibo-sec-dbt-bo-bo;isConvertible">
		<rdfs:label>is convertible</rdfs:label>
		<rdfs:domain rdf:resource="&fibo-sec-dbt-bo-bo;Bond"/>
		<rdfs:range rdf:resource="&xsd;boolean"/>
		<skos:definition xml:lang="en">has a conversion feature enabling it to be converted into another instrument on maturity</skos:definition>
	</owl:DatatypeProperty>
	
	<owl:ObjectProperty rdf:about="&fibo-sec-dbt-bo-bo;naked">
		<rdfs:label xml:lang="en">naked</rdfs:label>
		<rdfs:domain rdf:resource="&fibo-sec-dbt-bo-bo;Debenture"/>
		<rdfs:range rdf:resource="&fibo-fnd-utlx-val;TrueFalseValue"/>
		<skos:definition xml:lang="en">Whether the debenture is unsecured (Naked = Yes) or is secured (Naked = No).</skos:definition>
	</owl:ObjectProperty>
	
	<owl:ObjectProperty rdf:about="&fibo-sec-dbt-bo-bo;securitizationConditions">
		<rdfs:label xml:lang="en">securitization conditions</rdfs:label>
		<rdfs:domain rdf:resource="&fibo-sec-dbt-bo-bo;DebentureSecuritizationConditions"/>
		<rdfs:range rdf:resource="&fibo-fnd-utlx-val;TextValue"/>
		<skos:definition xml:lang="en">Textual description of the conditions for the securitization of the Debenture.</skos:definition>
	</owl:ObjectProperty>
	
	<owl:ObjectProperty rdf:about="&fibo-sec-dbt-bo-bo;securitizationConditions.1">
		<rdfs:subPropertyOf rdf:resource="&fibo-fnd-agr-ctr;hasContractualElement"/>
		<rdfs:label xml:lang="en">securitization conditions</rdfs:label>
		<rdfs:domain rdf:resource="&fibo-sec-dbt-bo-bo;Debenture"/>
		<rdfs:range rdf:resource="&fibo-sec-dbt-bo-bo;DebentureSecuritizationConditions"/>
	</owl:ObjectProperty>

</rdf:RDF>