<?xml version="1.0" encoding="UTF-8"?>
<!DOCTYPE rdf:RDF [
	<!ENTITY dct "http://purl.org/dc/terms/">
	<!ENTITY fibo-fnd-inf-inf "https://spec.edmcouncil.org/fibo/ontology/FND/InformationExt/InfoCore/">
	<!ENTITY fibo-fnd-inf-padr "https://spec.edmcouncil.org/fibo/ontology/FND/InformationExt/PostalAddress/">
	<!ENTITY fibo-fnd-oac-own "https://spec.edmcouncil.org/fibo/ontology/FND/OwnershipAndControl/Ownership/">
	<!ENTITY fibo-fnd-phy-phy "https://spec.edmcouncil.org/fibo/ontology/FND/PhysicalExt/Physical/">
	<!ENTITY fibo-fnd-plc-adr "https://spec.edmcouncil.org/fibo/ontology/FND/Places/Addresses/">
	<!ENTITY fibo-fnd-plc-loc "https://spec.edmcouncil.org/fibo/ontology/FND/Places/Locations/">
	<!ENTITY fibo-fnd-plcx-gph "https://spec.edmcouncil.org/fibo/ontology/FND/PlacesExt/Geophysical/">
	<!ENTITY fibo-fnd-plcx-re "https://spec.edmcouncil.org/fibo/ontology/FND/PlacesExt/RealEstate/">
	<!ENTITY fibo-fnd-rel-rel "https://spec.edmcouncil.org/fibo/ontology/FND/Relations/Relations/">
	<!ENTITY fibo-fnd-utl-av "https://spec.edmcouncil.org/fibo/ontology/FND/Utilities/AnnotationVocabulary/">
	<!ENTITY owl "http://www.w3.org/2002/07/owl#">
	<!ENTITY rdf "http://www.w3.org/1999/02/22-rdf-syntax-ns#">
	<!ENTITY rdfs "http://www.w3.org/2000/01/rdf-schema#">
	<!ENTITY skos "http://www.w3.org/2004/02/skos/core#">
	<!ENTITY xsd "http://www.w3.org/2001/XMLSchema#">
]>
<rdf:RDF xml:base="https://spec.edmcouncil.org/fibo/ontology/FND/PlacesExt/RealEstate/"
	xmlns:dct="http://purl.org/dc/terms/"
	xmlns:fibo-fnd-inf-inf="https://spec.edmcouncil.org/fibo/ontology/FND/InformationExt/InfoCore/"
	xmlns:fibo-fnd-inf-padr="https://spec.edmcouncil.org/fibo/ontology/FND/InformationExt/PostalAddress/"
	xmlns:fibo-fnd-oac-own="https://spec.edmcouncil.org/fibo/ontology/FND/OwnershipAndControl/Ownership/"
	xmlns:fibo-fnd-phy-phy="https://spec.edmcouncil.org/fibo/ontology/FND/PhysicalExt/Physical/"
	xmlns:fibo-fnd-plc-adr="https://spec.edmcouncil.org/fibo/ontology/FND/Places/Addresses/"
	xmlns:fibo-fnd-plc-loc="https://spec.edmcouncil.org/fibo/ontology/FND/Places/Locations/"
	xmlns:fibo-fnd-plcx-gph="https://spec.edmcouncil.org/fibo/ontology/FND/PlacesExt/Geophysical/"
	xmlns:fibo-fnd-plcx-re="https://spec.edmcouncil.org/fibo/ontology/FND/PlacesExt/RealEstate/"
	xmlns:fibo-fnd-rel-rel="https://spec.edmcouncil.org/fibo/ontology/FND/Relations/Relations/"
	xmlns:fibo-fnd-utl-av="https://spec.edmcouncil.org/fibo/ontology/FND/Utilities/AnnotationVocabulary/"
	xmlns:owl="http://www.w3.org/2002/07/owl#"
	xmlns:rdf="http://www.w3.org/1999/02/22-rdf-syntax-ns#"
	xmlns:rdfs="http://www.w3.org/2000/01/rdf-schema#"
	xmlns:skos="http://www.w3.org/2004/02/skos/core#"
	xmlns:xsd="http://www.w3.org/2001/XMLSchema#">
	
	<owl:Ontology rdf:about="https://spec.edmcouncil.org/fibo/ontology/FND/PlacesExt/RealEstate/">
		<rdfs:label xml:lang="en">RealEstate</rdfs:label>
		<dct:abstract>Defines the notion of real estate. This draws on a combination of geophysical (land parcel) and built environment concepts, and also allows for the use of leasehold contracts as collateral in mortgages as a kind of real estate asset. 
		This model is considerably more complex and conceptual than the published Release ontology for real estate, which defines it merely as some kind of location. Some of these concepts will be needed in defining details about mortgage loans and other applications of collateral.</dct:abstract>
		<owl:imports rdf:resource="https://spec.edmcouncil.org/fibo/ontology/FND/InformationExt/AddressExtensions/"/>
		<owl:imports rdf:resource="https://spec.edmcouncil.org/fibo/ontology/FND/InformationExt/InfoCore/"/>
		<owl:imports rdf:resource="https://spec.edmcouncil.org/fibo/ontology/FND/InformationExt/PostalAddress/"/>
		<owl:imports rdf:resource="https://spec.edmcouncil.org/fibo/ontology/FND/OwnershipAndControl/Ownership/"/>
		<owl:imports rdf:resource="https://spec.edmcouncil.org/fibo/ontology/FND/PhysicalExt/Physical/"/>
		<owl:imports rdf:resource="https://spec.edmcouncil.org/fibo/ontology/FND/Places/Addresses/"/>
		<owl:imports rdf:resource="https://spec.edmcouncil.org/fibo/ontology/FND/Places/Locations/"/>
		<owl:imports rdf:resource="https://spec.edmcouncil.org/fibo/ontology/FND/PlacesExt/Geophysical/"/>
		<owl:imports rdf:resource="https://spec.edmcouncil.org/fibo/ontology/FND/Relations/Relations/"/>
		<owl:imports rdf:resource="https://spec.edmcouncil.org/fibo/ontology/FND/Utilities/AnnotationVocabulary/"/>
		<owl:versionIRI rdf:resource="https://spec.edmcouncil.org/fibo/ontology/FND/PlacesExt/RealEstate/"/>
		<fibo-fnd-utl-av:hasMaturityLevel rdf:resource="&fibo-fnd-utl-av;Informative"/>
	</owl:Ontology>
	
	<owl:Class rdf:about="&fibo-fnd-plc-adr;PhysicalAddress">
		<rdfs:subClassOf>
			<owl:Restriction>
				<owl:onProperty rdf:resource="&fibo-fnd-inf-padr;isOf"/>
				<owl:someValuesFrom rdf:resource="&fibo-fnd-plc-loc;RealEstate"/>
			</owl:Restriction>
		</rdfs:subClassOf>
	</owl:Class>
	
	<owl:Class rdf:about="&fibo-fnd-plc-loc;RealEstate">
		<rdfs:subClassOf rdf:resource="&fibo-fnd-plc-loc;PhysicalLocation"/>
		<rdfs:subClassOf>
			<owl:Restriction>
				<owl:onProperty rdf:resource="&fibo-fnd-plcx-re;realEstateCoextensiveWith"/>
				<owl:someValuesFrom>
					<owl:Class>
						<owl:unionOf rdf:parseType="Collection">
							<rdf:Description rdf:about="&fibo-fnd-plcx-gph;LandParcel">
							</rdf:Description>
							<rdf:Description rdf:about="&fibo-fnd-plcx-re;BuiltProperty">
							</rdf:Description>
						</owl:unionOf>
					</owl:Class>
				</owl:someValuesFrom>
			</owl:Restriction>
		</rdfs:subClassOf>
		<rdfs:subClassOf>
			<owl:Restriction>
				<owl:onProperty rdf:resource="&fibo-fnd-plcx-re;realEstateOwnedBy"/>
				<owl:someValuesFrom rdf:resource="&fibo-fnd-plcx-re;PropertyOwner"/>
			</owl:Restriction>
		</rdfs:subClassOf>
		<rdfs:subClassOf>
			<owl:Restriction>
				<owl:onProperty rdf:resource="&fibo-fnd-rel-rel;hasPart"/>
				<owl:someValuesFrom rdf:resource="&fibo-fnd-plc-loc;RealEstate"/>
			</owl:Restriction>
		</rdfs:subClassOf>
		<skos:definition xml:lang="en">Land plus anything permanently fixed to it, including buildings, sheds and other items attached to the structure. Explanatory Note: Although, media often refers to the &quot;real estate market&quot; from the perspective of residential living, real estate can be grouped into three broad categories based on its use, namely residential, commercial and industrial. Explanatory Note: Examples of real estate include undeveloped land, houses, condominiums, townhomes, office buildings, retail store buildings and factories. Scope Note: Bricks and mortar or land which can be owned.</skos:definition>
	</owl:Class>
	
	<owl:Class rdf:about="&fibo-fnd-plcx-re;Apartment">
		<rdfs:subClassOf rdf:resource="&fibo-fnd-plcx-re;BuildingSubUnit"/>
		<rdfs:subClassOf>
			<owl:Restriction>
				<owl:onProperty rdf:resource="&fibo-fnd-inf-padr;apartmentIdentifiedBy"/>
				<owl:someValuesFrom rdf:resource="&fibo-fnd-inf-padr;BuildingSubUnitAddressFragment"/>
			</owl:Restriction>
		</rdfs:subClassOf>
		<rdfs:label xml:lang="en">apartment</rdfs:label>
		<skos:definition xml:lang="en">A building subbdivision intended for habitation.</skos:definition>
	</owl:Class>
	
	<owl:Class rdf:about="&fibo-fnd-plcx-re;Building">
		<rdfs:subClassOf rdf:resource="&fibo-fnd-plcx-re;BuiltProperty"/>
		<rdfs:subClassOf>
			<owl:Restriction>
				<owl:onProperty rdf:resource="&fibo-fnd-inf-padr;buildingIdentifiedBy"/>
				<owl:someValuesFrom rdf:resource="&fibo-fnd-inf-padr;StreetAddressText"/>
			</owl:Restriction>
		</rdfs:subClassOf>
		<rdfs:subClassOf>
			<owl:Restriction>
				<owl:onProperty rdf:resource="&fibo-fnd-rel-rel;hasPart"/>
				<owl:someValuesFrom rdf:resource="&fibo-fnd-plcx-re;BuildingSubUnit"/>
			</owl:Restriction>
		</rdfs:subClassOf>
		<rdfs:label xml:lang="en">building</rdfs:label>
		<skos:definition xml:lang="en">A discrete construction on its own foundations or pilings.</skos:definition>
	</owl:Class>
	
	<owl:Class rdf:about="&fibo-fnd-plcx-re;BuildingSubUnit">
		<rdfs:subClassOf rdf:resource="&fibo-fnd-plcx-re;BuiltProperty"/>
		<rdfs:label xml:lang="en">building sub unit</rdfs:label>
		<skos:definition xml:lang="en">A discrete subdivision of some Building.</skos:definition>
	</owl:Class>
	
	<owl:Class rdf:about="&fibo-fnd-plcx-re;BuiltProperty">
		<rdfs:subClassOf rdf:resource="&fibo-fnd-phy-phy;DiscretePhysicalThing"/>
		<rdfs:subClassOf>
			<owl:Restriction>
				<owl:onProperty rdf:resource="&fibo-fnd-plcx-re;hasLocation"/>
				<owl:someValuesFrom rdf:resource="&fibo-fnd-plcx-gph;GeophysicalLocation"/>
			</owl:Restriction>
		</rdfs:subClassOf>
		<rdfs:label xml:lang="en">built property</rdfs:label>
		<skos:definition xml:lang="en">Something which is constructed via construction methods; bricks and mortar.</skos:definition>
	</owl:Class>
	
	<owl:Class rdf:about="&fibo-fnd-plcx-re;Floor">
		<rdfs:subClassOf rdf:resource="&fibo-fnd-plcx-re;BuildingSubUnit"/>
		<rdfs:subClassOf>
			<owl:Restriction>
				<owl:onProperty rdf:resource="&fibo-fnd-inf-padr;floorIdentifiedBy"/>
				<owl:someValuesFrom rdf:resource="&fibo-fnd-inf-padr;BuildingSubUnitAddressFragment"/>
			</owl:Restriction>
		</rdfs:subClassOf>
		<rdfs:label xml:lang="en">floor</rdfs:label>
		<skos:definition xml:lang="en">A building subdivision whose extent is the horizontal extent of the building at that height.</skos:definition>
	</owl:Class>
	
	<owl:Class rdf:about="&fibo-fnd-plcx-re;PropertyOwner">
		<rdfs:subClassOf rdf:resource="&fibo-fnd-oac-own;Owner"/>
		<rdfs:label xml:lang="en">property owner</rdfs:label>
	</owl:Class>
	
	<owl:Class rdf:about="&fibo-fnd-plcx-re;Suite">
		<rdfs:subClassOf rdf:resource="&fibo-fnd-plcx-re;BuildingSubUnit"/>
		<rdfs:subClassOf>
			<owl:Restriction>
				<owl:onProperty rdf:resource="&fibo-fnd-inf-padr;suiteIdentifiedBy"/>
				<owl:someValuesFrom rdf:resource="&fibo-fnd-inf-padr;BuildingSubUnitAddressFragment"/>
			</owl:Restriction>
		</rdfs:subClassOf>
		<rdfs:label xml:lang="en">suite</rdfs:label>
		<skos:definition xml:lang="en">A subdivision of a building for which the purposes are not clearly defined or may be variable, generally consisting of a number of contiguous rooms on one or more floors.</skos:definition>
	</owl:Class>
	
	<owl:ObjectProperty rdf:about="&fibo-fnd-plcx-re;hasLocation">
		<rdfs:label xml:lang="en">has location</rdfs:label>
		<rdfs:domain rdf:resource="&fibo-fnd-plcx-re;BuiltProperty"/>
		<rdfs:range rdf:resource="&fibo-fnd-plcx-gph;GeophysicalLocation"/>
		<skos:definition xml:lang="en">The physical location of the built item or property.</skos:definition>
	</owl:ObjectProperty>
	
	<owl:ObjectProperty rdf:about="&fibo-fnd-plcx-re;identifiedBy">
		<rdfs:subPropertyOf rdf:resource="&fibo-fnd-inf-inf;details"/>
		<rdfs:label xml:lang="en">identified by</rdfs:label>
		<rdfs:domain rdf:resource="&fibo-fnd-plc-loc;RealEstate"/>
		<rdfs:range rdf:resource="&fibo-fnd-plc-adr;PhysicalAddress"/>
	</owl:ObjectProperty>
	
	<owl:DatatypeProperty rdf:about="&fibo-fnd-plcx-re;leasehold">
		<rdfs:label xml:lang="en">leasehold</rdfs:label>
		<rdfs:domain rdf:resource="&fibo-fnd-plc-loc;RealEstate"/>
		<rdfs:range rdf:resource="&xsd;boolean"/>
		<skos:definition xml:lang="en">Typically a leasehold is where the land is not owned by the borrower, rather it is leased from a third party for a term that exceeds the life of the mortgage.</skos:definition>
	</owl:DatatypeProperty>
	
	<owl:ObjectProperty rdf:about="&fibo-fnd-plcx-re;realEstateCoextensiveWith">
		<rdfs:label xml:lang="en">real estate coextensive with</rdfs:label>
		<rdfs:domain rdf:resource="&fibo-fnd-plc-loc;RealEstate"/>
		<rdfs:range>
			<owl:Class>
				<owl:unionOf rdf:parseType="Collection">
					<rdf:Description rdf:about="&fibo-fnd-plcx-gph;LandParcel">
					</rdf:Description>
					<rdf:Description rdf:about="&fibo-fnd-plcx-re;BuiltProperty">
					</rdf:Description>
				</owl:unionOf>
			</owl:Class>
		</rdfs:range>
		<skos:definition xml:lang="en">Real Estate corresponds to either some built item or some parcel of land.</skos:definition>
		<skos:scopeNote xml:lang="en">This is represented as a logical union of Built Item and Land Parcel. Scope Note: Future changes in Real Estate ontology alignment may well change or elaborate on this.</skos:scopeNote>
	</owl:ObjectProperty>
	
	<owl:ObjectProperty rdf:about="&fibo-fnd-plcx-re;realEstateOwnedBy">
		<rdfs:label xml:lang="en">real estate owned by</rdfs:label>
		<rdfs:domain rdf:resource="&fibo-fnd-plc-loc;RealEstate"/>
		<rdfs:range rdf:resource="&fibo-fnd-plcx-re;PropertyOwner"/>
	</owl:ObjectProperty>

</rdf:RDF>