<?xml version="1.0" encoding="UTF-8"?>
  
<!DOCTYPE rdf:RDF [
    <!ENTITY fibo-be-le-fbo "http://spec.edmcouncil.org/fibo/red/be/legal-entities/formal-business-organizations/">
    <!ENTITY fibo-fnd-info-sch "http://spec.edmcouncil.org/fibo/red/fnd/information/schemes/">
    <!ENTITY fibo-fnd-info-ids "http://spec.edmcouncil.org/fibo/red/fnd/information/identifiers/">
    <!ENTITY fibo-fnd-pty-pty "http://spec.edmcouncil.org/fibo/red/fnd/parties/parties/">
    <!ENTITY fibo-fnd-plc-adr "http://spec.edmcouncil.org/fibo/red/fnd/places/addresses/">
    <!ENTITY fibo-fnd-org-fm "http://spec.edmcouncil.org/fibo/red/fnd/organizations/formal-organizations/">
    <!ENTITY fibo-fnd-org-org "http://spec.edmcouncil.org/fibo/red/fnd/organizations/organizations/">
    <!ENTITY fibo-fnd-utl-bt "http://spec.edmcouncil.org/fibo/red/fnd/utilities/business-facing-types/">
    <!ENTITY fibo-fnd-acc-aeq "http://spec.edmcouncil.org/fibo/red/fnd/accounting/accounting-equity/">
    <!ENTITY fibo-be-le-lp "http://spec.edmcouncil.org/fibo/red/be/legal-entities/legal-persons/">
    <!ENTITY fibo-fnd-rel-rel "http://spec.edmcouncil.org/fibo/red/fnd/relations/relations/">
    <!ENTITY fibo-fnd-pty-rl "http://spec.edmcouncil.org/fibo/red/fnd/parties/roles/">
    <!ENTITY fibo-fnd-agr-ctr "http://spec.edmcouncil.org/fibo/red/fnd/agreements/contracts/">
]>

<rdf:RDF xmlns:xsd="http://www.w3.org/2001/XMLSchema#"
         xmlns:sm="http://www.omg.org/techprocess/ab/SpecificationMetadata/"
         xmlns:xs="http://www.w3.org/2001/XMLSchema"
         xmlns:fibo-fnd-utl-av="http://www.omg.org/spec/EDMC-FIBO/FND/Utilities/AnnotationVocabulary/"
         xmlns:rdf="http://www.w3.org/1999/02/22-rdf-syntax-ns#"
         xmlns:rdfs="http://www.w3.org/2000/01/rdf-schema#"
         xmlns:owl="http://www.w3.org/2002/07/owl#"
         xmlns:skos="http://www.w3.org/2004/02/skos/core#"
         xmlns:dc="http://purl.org/dc/terms/"
         xml:base="http://spec.edmcouncil.org/fibo/red/be/legal-entities/formal-business-organizations/">

   <owl:Ontology rdf:about="http://spec.edmcouncil.org/fibo/red/be/legal-entities/formal-business-organizations/">
      <owl:imports rdf:resource="http://spec.edmcouncil.org/fibo/red/fnd/information/schemes/"/>
      <owl:imports rdf:resource="http://spec.edmcouncil.org/fibo/red/fnd/information/identifiers/"/>
      <owl:imports rdf:resource="http://spec.edmcouncil.org/fibo/red/fnd/parties/parties/"/>
      <owl:imports rdf:resource="http://spec.edmcouncil.org/fibo/red/fnd/places/addresses/"/>
      <owl:imports rdf:resource="http://spec.edmcouncil.org/fibo/red/fnd/organizations/formal-organizations/"/>
      <owl:imports rdf:resource="http://spec.edmcouncil.org/fibo/red/fnd/organizations/organizations/"/>
      <owl:imports rdf:resource="http://spec.edmcouncil.org/fibo/red/fnd/utilities/business-facing-types/"/>
      <owl:imports rdf:resource="http://spec.edmcouncil.org/fibo/red/fnd/accounting/accounting-equity/"/>
      <owl:imports rdf:resource="http://spec.edmcouncil.org/fibo/red/be/legal-entities/legal-persons/"/>
      <owl:imports rdf:resource="http://spec.edmcouncil.org/fibo/red/fnd/relations/relations/"/>
      <owl:imports rdf:resource="http://spec.edmcouncil.org/fibo/red/fnd/parties/roles/"/>
      <owl:imports rdf:resource="http://spec.edmcouncil.org/fibo/red/fnd/agreements/contracts/"/>
   </owl:Ontology>


  <!--
    ///////////////////////////////////////////////////////////////////////////////////////
    //
    // Datatypes
    //
    ///////////////////////////////////////////////////////////////////////////////////////
    -->



  <!--
    ///////////////////////////////////////////////////////////////////////////////////////
    //
    // Object Properties
    //
    ///////////////////////////////////////////////////////////////////////////////////////
    -->


<owl:ObjectProperty rdf:about="&fibo-be-le-fbo;formalBusinessOrganizationIsMemberOf">
      <rdfs:label>formal business organization is member of</rdfs:label>
      <rdfs:subPropertyOf rdf:resource="&fibo-fnd-rel-rel;isMemberOf"/>
      <rdfs:subPropertyOf rdf:resource="&fibo-fnd-pty-rl;hasRole"/>
      <rdfs:domain rdf:resource="&fibo-be-le-fbo;FormalBusinessOrganizationMember"/>
      <rdfs:range rdf:resource="&fibo-be-le-fbo;FormallyConstitutedOrganization"/>
   </owl:ObjectProperty>

   <owl:ObjectProperty rdf:about="&fibo-be-le-fbo;hasSectorClassification">
      <rdfs:label>has sector classification</rdfs:label>
      <rdfs:subPropertyOf rdf:resource="&fibo-fnd-rel-rel;isClassifiedBy"/>
      <rdfs:domain rdf:resource="&fibo-be-le-fbo;FormallyConstitutedOrganization"/>
      <rdfs:range rdf:resource="&fibo-be-le-fbo;OrganizationIndustrySectorClassification"/>
      <owl:inverseOf rdf:resource="&fibo-be-le-fbo;organizatonIndustrySectorClassificaitonClassifies"/>
   </owl:ObjectProperty>

   <owl:ObjectProperty rdf:about="&fibo-be-le-fbo;formallyConstitutedOrganizationIsGovernedBy">
      <rdfs:label>formally constituted organization is governed by</rdfs:label>
      <skos:definition>The or any agreement which governs the relationships among the principals in some formal organization.</skos:definition>
      <rdfs:subPropertyOf rdf:resource="&fibo-fnd-rel-rel;isGoverneBy"/>
      <rdfs:domain rdf:resource="&fibo-be-le-fbo;FormallyConstitutedOrganization"/>
      <rdfs:range rdf:resource="&fibo-be-le-fbo;OrganizationCoveringAgreement"/>
   </owl:ObjectProperty>

   <owl:ObjectProperty rdf:about="&fibo-be-le-fbo;formallyConstitutedOrganizationIsIdentifiedBy">
      <rdfs:label>formally constituted organization is identified by</rdfs:label>
      <skos:definition>A formal, published identifier of the business entity.</skos:definition>
      <rdfs:subPropertyOf rdf:resource="&fibo-fnd-info-ids;hasIdentifier"/>
      <rdfs:subPropertyOf rdf:resource="&fibo-fnd-rel-rel;isIdentifiedBy"/>
      <rdfs:domain rdf:resource="&fibo-be-le-fbo;FormallyConstitutedOrganization"/>
      <rdfs:range rdf:resource="&fibo-be-le-fbo;OrganizationIdentificationCode"/>
   </owl:ObjectProperty>

   <owl:ObjectProperty rdf:about="&fibo-be-le-fbo;defines">
      <rdfs:label>defines</rdfs:label>
      <skos:definition>An organization identification code defined in the scheme.</skos:definition>
      <rdfs:subPropertyOf rdf:resource="&fibo-fnd-rel-rel;defines"/>
      <rdfs:subPropertyOf rdf:resource="&fibo-fnd-info-ids;defines"/>
      <rdfs:domain rdf:resource="&fibo-be-le-fbo;OrganizationIdentificationScheme"/>
      <rdfs:range rdf:resource="&fibo-be-le-fbo;OrganizationIdentificationCode"/>
   </owl:ObjectProperty>

   <owl:ObjectProperty rdf:about="&fibo-be-le-fbo;organizatonIndustrySectorClassificaitonClassifies">
      <rdfs:label>organizaton industry sector classificaiton classifies</rdfs:label>
      <skos:definition>A business entity which is covered by the classification.</skos:definition>
      <rdfs:subPropertyOf rdf:resource="&fibo-fnd-rel-rel;classifies"/>
      <rdfs:subPropertyOf rdf:resource="&fibo-fnd-info-sch;classifies"/>
      <rdfs:domain rdf:resource="&fibo-be-le-fbo;OrganizationIndustrySectorClassification"/>
      <rdfs:range rdf:resource="&fibo-be-le-fbo;FormallyConstitutedOrganization"/>
   </owl:ObjectProperty>

   <owl:ObjectProperty rdf:about="&fibo-be-le-fbo;hasInternalEntity">
      <rdfs:label>has internal entity</rdfs:label>
      <skos:definition>The organization has some part which is formally defined as an Internal Entity, for example for reporting, management or accounting purposes.</skos:definition>
      <rdfs:subPropertyOf rdf:resource="&fibo-be-le-fbo;hasSubUnit"/>
      <rdfs:domain rdf:resource="&fibo-be-le-fbo;FormallyConstitutedOrganization"/>
      <rdfs:range rdf:resource="&fibo-be-le-fbo;OrganizationalSubUnit"/>
   </owl:ObjectProperty>

   <owl:ObjectProperty rdf:about="&fibo-be-le-fbo;hasSubUnit">
      <rdfs:label>has sub unit</rdfs:label>
      <rdfs:subPropertyOf rdf:resource="&fibo-fnd-rel-rel;hasPart"/>
      <rdfs:domain rdf:resource="&fibo-be-le-fbo;FormallyConstitutedOrganization"/>
      <rdfs:range rdf:resource="&fibo-be-le-fbo;OrganizationalSubUnit"/>
      <owl:inverseOf rdf:resource="&fibo-be-le-fbo;isSubUnitOf"/>
   </owl:ObjectProperty>

   <owl:ObjectProperty rdf:about="&fibo-be-le-fbo;hasEquity">
      <rdfs:label>has equity</rdfs:label>
      <skos:definition>The Formal Organization has some form of Stockholder Equity.</skos:definition>
      <rdfs:domain rdf:resource="&fibo-be-le-fbo;FormallyConstitutedOrganization"/>
      <rdfs:range rdf:resource="&fibo-fnd-acc-aeq;StockholdersEquity"/>
   </owl:ObjectProperty>

   <owl:ObjectProperty rdf:about="&fibo-be-le-fbo;hasOperatingAddress">
      <rdfs:label>has operating address</rdfs:label>
      <skos:definition>Address at which the organization carries out its operations.</skos:definition>
      <rdfs:subPropertyOf rdf:resource="&fibo-fnd-org-org;organizationHasAddress"/>
      <rdfs:domain rdf:resource="&fibo-be-le-fbo;FormallyConstitutedOrganization"/>
      <rdfs:range rdf:resource="&fibo-fnd-plc-adr;PostalAddress"/>
   </owl:ObjectProperty>

   <owl:ObjectProperty rdf:about="&fibo-be-le-fbo;hasPrimaryAddress">
      <rdfs:label>has primary address</rdfs:label>
      <skos:definition>The main address at which communications to the organization may be addressed; its headquarters address.</skos:definition>
      <rdfs:subPropertyOf rdf:resource="&fibo-fnd-org-org;organizationHasAddress"/>
      <rdfs:domain rdf:resource="&fibo-be-le-fbo;FormallyConstitutedOrganization"/>
      <rdfs:range rdf:resource="&fibo-fnd-plc-adr;PostalAddress"/>
   </owl:ObjectProperty>

   <owl:ObjectProperty rdf:about="&fibo-be-le-fbo;hasRegisteredAddress">
      <rdfs:label>has registered address</rdfs:label>
      <skos:definition>The organization has an address at which it is registered and at which legal papers may be served on it.</skos:definition>
      <rdfs:subPropertyOf rdf:resource="&fibo-fnd-org-org;organizationHasAddress"/>
      <rdfs:domain rdf:resource="&fibo-be-le-fbo;FormallyConstitutedOrganization"/>
      <rdfs:range rdf:resource="&fibo-be-le-fbo;RegisteredAddress"/>
   </owl:ObjectProperty>

   <owl:ObjectProperty rdf:about="&fibo-be-le-fbo;hasSignatory">
      <rdfs:label>has signatory</rdfs:label>
      <skos:definition>has a party which is authorized to sign contracts on the party of the entity.</skos:definition>
      <rdfs:subPropertyOf rdf:resource="&fibo-fnd-pty-pty;hasPartyInRole"/>
      <rdfs:domain rdf:resource="&fibo-be-le-fbo;FormallyConstitutedOrganization"/>
      <rdfs:range rdf:resource="&fibo-be-le-lp;Signatory"/>
   </owl:ObjectProperty>

   <owl:ObjectProperty rdf:about="&fibo-be-le-fbo;isSubUnitOf">
      <rdfs:label>is sub unit of</rdfs:label>
      <skos:definition>The organization is a sub-unit of a Formal Organization and has the role and function of being a formal part of that organization, such as a branch.</skos:definition>
      <rdfs:subPropertyOf rdf:resource="&fibo-fnd-rel-rel;isPartOf"/>
      <rdfs:domain rdf:resource="&fibo-be-le-fbo;OrganizationalSubUnit"/>
      <rdfs:range rdf:resource="&fibo-be-le-fbo;FormallyConstitutedOrganization"/>
   </owl:ObjectProperty>


  <!--
    ///////////////////////////////////////////////////////////////////////////////////////
    //
    // Data Properties
    //
    ///////////////////////////////////////////////////////////////////////////////////////
    -->


<owl:DatatypeProperty rdf:about="&fibo-be-le-fbo;hasUniqueIdentifier">
      <rdfs:label>has unique identifier</rdfs:label>
      <skos:definition>links an entity to a unique identifier for that entity; may be associated with anything. With reference to a given (possibly implicit) set of objects, a unique identifier (UID) is any identifier which is guaranteed to be unique among all identifiers used for those objects and for a specific purpose. Editorial Note: Review this definition since it seems to assert unique by purpose and object alone; uniqueness can only be guaranteed by scheme.</skos:definition>
      <rdfs:range rdf:resource="&fibo-fnd-utl-bt;text"/>
   </owl:DatatypeProperty>


  <!--
    ///////////////////////////////////////////////////////////////////////////////////////
    //
    // Annotation Properties
    //
    ///////////////////////////////////////////////////////////////////////////////////////
    -->



  <!--
    ///////////////////////////////////////////////////////////////////////////////////////
    //
    // Classes
    //
    ///////////////////////////////////////////////////////////////////////////////////////
    -->


<owl:Class rdf:about="&fibo-be-le-fbo;Branch">
      <rdfs:label>branch</rdfs:label>
      <skos:definition>A part of a business organization or company, identified as a branch.</skos:definition>
      <rdfs:subClassOf rdf:resource="&fibo-be-le-fbo;OrganizationalSubUnit"/>
   </owl:Class>

   <owl:Class rdf:about="&fibo-be-le-fbo;Division">
      <rdfs:label>division</rdfs:label>
      <skos:definition>A part of a company.</skos:definition>
   </owl:Class>

   <owl:Class rdf:about="&fibo-be-le-fbo;FormalBusinessOrganizationMember">
      <rdfs:label>formal business organization member</rdfs:label>
      <skos:definition>A member of some Formal Organization.</skos:definition>
      <rdfs:subClassOf rdf:resource="&fibo-fnd-pty-pty;OrganizationMember"/>
   </owl:Class>

   <owl:Class rdf:about="&fibo-be-le-fbo;JointVenture">
      <rdfs:label>joint venture</rdfs:label>
      <skos:definition>A formal venture between two or more business entities.</skos:definition>
      <rdfs:subClassOf rdf:resource="&fibo-be-le-fbo;FormallyConstitutedOrganization"/>
   </owl:Class>

   <owl:Class rdf:about="&fibo-be-le-fbo;OrganizationCoveringAgreement">
      <rdfs:label>organization covering agreement</rdfs:label>
      <skos:definition>A formal agreement between the principals in a formal organization which covers the relationship between the principals, and between the principals and the entity.</skos:definition>
      <rdfs:subClassOf rdf:resource="&fibo-fnd-agr-ctr;WrittenContract"/>
   </owl:Class>

   <owl:Class rdf:about="&fibo-be-le-fbo;OrganizationIdentificationScheme">
      <rdfs:label>organization identification scheme</rdfs:label>
      <skos:definition>A formal scheme defining identification codes for a business entity.</skos:definition>
      <rdfs:subClassOf rdf:resource="&fibo-fnd-info-ids;IdentificationScheme"/>
   </owl:Class>

   <owl:Class rdf:about="&fibo-be-le-fbo;OrganizationIndustrySectorClassification">
      <rdfs:label>organization industry sector classification</rdfs:label>
      <skos:definition>The classification of an organization in terms of the industry sector in which it carries out business.</skos:definition>
      <rdfs:subClassOf rdf:resource="&fibo-fnd-info-sch;Classification"/>
   </owl:Class>

   <owl:Class rdf:about="&fibo-be-le-fbo;OrganizationalSubUnit">
      <rdfs:label>organizational sub unit</rdfs:label>
      <skos:definition>An Organization which is part of some larger Formal Organization and only has full recognition within the context of that Formal Organization, it is not a Legal Entity in its own right.</skos:definition>
      <rdfs:subClassOf rdf:resource="&fibo-fnd-org-fm;FormalOrganization"/>
   </owl:Class>

   <owl:Class rdf:about="&fibo-be-le-fbo;RegisteredAddress">
      <rdfs:label>registered address</rdfs:label>
      <skos:definition>The address at which an entity is registered and at which legal papers may be served.</skos:definition>
      <rdfs:subClassOf rdf:resource="&fibo-fnd-plc-adr;PostalAddress"/>
   </owl:Class>

   <owl:Class rdf:about="&fibo-be-le-fbo;OrganizationIdentificationCode">
      <rdfs:label>organization identification code</rdfs:label>
      <skos:definition>A textual code which uniquely identifies a formal organization Further Notes Things which may identified by this kind of code Include but are not restricted to Legal Entity. At this most general level, this may be the identifier for a Fund, for a Legal Entity, for a Trust, or for the LEI scope of "Artificial Person plus Trust".</skos:definition>
      <rdfs:subClassOf rdf:resource="&fibo-fnd-info-ids;Identifier"/>
   </owl:Class>

   <owl:Class rdf:about="&fibo-be-le-fbo;FormallyConstitutedOrganization">
      <rdfs:label>formally constituted organization</rdfs:label>
      <skos:definition>Any organization with some formal contractual agreement among its principals.</skos:definition>
   </owl:Class>


  <!--
    ///////////////////////////////////////////////////////////////////////////////////////
    //
    // Individuals
    //
    ///////////////////////////////////////////////////////////////////////////////////////
    -->


</rdf:RDF>