<?xml version="1.0" encoding="UTF-8"?>
<rdf:RDF xmlns:xsd="http://www.w3.org/2001/XMLSchema#"
         xmlns:sm="http://www.omg.org/techprocess/ab/SpecificationMetadata/"
         xmlns:fibo-fnd-utl-av="http://www.omg.org/spec/EDMC-FIBO/FND/Utilities/AnnotationVocabulary/"
         xmlns:rdf="http://www.w3.org/1999/02/22-rdf-syntax-ns#"
         xmlns:rdfs="http://www.w3.org/2000/01/rdf-schema#"
         xmlns:owl="http://www.w3.org/2002/07/owl#"
         xmlns:skos="http://www.w3.org/2004/02/skos/core#"
         xmlns:dc="http://purl.org/dc/terms/"
         xml:base="http://www.edmcouncil.org/spec/EDMC-SR/FND/AgreementsExt/ContractElements/">

   <owl:Ontology rdf:about="http://www.edmcouncil.org/spec/EDMC-SR/FND/AgreementsExt/ContractElements/">
      <owl:imports rdf:resource="http://www.omg.org/spec/EDMC-SR/FND/Agreements/Contracts/"/>
   </owl:Ontology>

   <!--Datatypes-->

<!--Object Properties-->

<owl:ObjectProperty rdf:about="http://www.edmcouncil.org/spec/EDMC-SR/FND/AgreementsExt/ContractElements/IdentifiesContractPartyAs">
      <skos:definition>The business entities identified in the contact party identification.</skos:definition>
      <rdfs:domain rdf:resource="http://www.edmcouncil.org/spec/EDMC-SR/FND/AgreementsExt/ContractElements/ContractPartyIdentification"/>
      <rdfs:range rdf:resource="http://www.omg.org/spec/EDMC-SR/BE/LegalEntities/LEIEntities/ContractuallyCapableEntity"/>
   </owl:ObjectProperty>

   <owl:ObjectProperty rdf:about="http://www.edmcouncil.org/spec/EDMC-SR/FND/AgreementsExt/ContractElements/clauseContainsTerm">
      <skos:definition>An individual term contained within the clause.</skos:definition>
      <rdfs:subPropertyOf rdf:resource="http://www.edmcouncil.org/spec/EDMC-SR/FND/AgreementsExt/ContractElements/writtenContractHasPart"/>
      <rdfs:domain rdf:resource="http://www.edmcouncil.org/spec/EDMC-SR/FND/AgreementsExt/ContractElements/ContractClause"/>
      <rdfs:range rdf:resource="http://www.edmcouncil.org/spec/EDMC-SR/FND/AgreementsExt/ContractElements/ContractTerm"/>
   </owl:ObjectProperty>

   <owl:ObjectProperty rdf:about="http://www.edmcouncil.org/spec/EDMC-SR/FND/AgreementsExt/ContractElements/identifies">
      <skos:definition>A party identified in the contract party identification.</skos:definition>
      <rdfs:subPropertyOf rdf:resource="http://www.edmcouncil.org/spec/EDMC-SR/FND/Information/Identification/identifies"/>
      <rdfs:domain rdf:resource="http://www.edmcouncil.org/spec/EDMC-SR/FND/AgreementsExt/ContractElements/ContractPartyIdentification"/>
      <rdfs:range rdf:resource="http://www.edmcouncil.org/spec/EDMC-SR/FND/AgreementsExt/ContractsExtensions/ContractParty"/>
   </owl:ObjectProperty>

   <owl:ObjectProperty rdf:about="http://www.edmcouncil.org/spec/EDMC-SR/FND/AgreementsExt/ContractElements/definesPrincipals">
      <skos:definition>The identification of parties to the contract as embodied in the preamble.</skos:definition>
      <rdfs:domain rdf:resource="http://www.edmcouncil.org/spec/EDMC-SR/FND/AgreementsExt/ContractElements/ContractPreamble"/>
      <rdfs:range rdf:resource="http://www.edmcouncil.org/spec/EDMC-SR/FND/AgreementsExt/ContractElements/ContractPrincipalsIdentification"/>
   </owl:ObjectProperty>

   <owl:ObjectProperty rdf:about="http://www.edmcouncil.org/spec/EDMC-SR/FND/AgreementsExt/ContractElements/identifiesPrincipal">
      <skos:definition>The principal to the contract, identified in the contract principals identification.</skos:definition>
      <rdfs:subPropertyOf rdf:resource="http://www.edmcouncil.org/spec/EDMC-SR/FND/AgreementsExt/ContractElements/identifies"/>
      <rdfs:domain rdf:resource="http://www.edmcouncil.org/spec/EDMC-SR/FND/AgreementsExt/ContractElements/ContractPrincipalsIdentification"/>
      <rdfs:range rdf:resource="http://www.omg.org/spec/EDMC-SR/FND/Agreements/Contracts/ContractPrincipal"/>
   </owl:ObjectProperty>

   <owl:ObjectProperty rdf:about="http://www.edmcouncil.org/spec/EDMC-SR/FND/AgreementsExt/ContractElements/identifiesCounterparty">
      <skos:definition>The counterparty to the contract, identified in the contract principals identification.</skos:definition>
      <rdfs:subPropertyOf rdf:resource="http://www.edmcouncil.org/spec/EDMC-SR/FND/AgreementsExt/ContractElements/identifies"/>
      <rdfs:domain rdf:resource="http://www.edmcouncil.org/spec/EDMC-SR/FND/AgreementsExt/ContractElements/ContractPrincipalsIdentification"/>
      <rdfs:range rdf:resource="http://www.omg.org/spec/EDMC-SR/FND/Agreements/Contracts/ContractCounterparty"/>
   </owl:ObjectProperty>

   <owl:ObjectProperty rdf:about="http://www.edmcouncil.org/spec/EDMC-SR/FND/AgreementsExt/ContractElements/hasTerm">
      <skos:definition>An individual term within the contractual terms set.</skos:definition>
      <rdfs:domain rdf:resource="http://www.omg.org/spec/EDMC-SR/FND/Agreements/Contracts/ContractTermsSet"/>
      <rdfs:range rdf:resource="http://www.edmcouncil.org/spec/EDMC-SR/FND/AgreementsExt/ContractElements/ContractTerm"/>
   </owl:ObjectProperty>

   <owl:ObjectProperty rdf:about="http://www.edmcouncil.org/spec/EDMC-SR/FND/AgreementsExt/ContractElements/identifiesThirdParty">
      <skos:definition>A third party identified in the third party identification.</skos:definition>
      <rdfs:subPropertyOf rdf:resource="http://www.edmcouncil.org/spec/EDMC-SR/FND/AgreementsExt/ContractElements/identifies"/>
      <rdfs:domain rdf:resource="http://www.edmcouncil.org/spec/EDMC-SR/FND/AgreementsExt/ContractElements/ContractThirdPartyIdentification"/>
      <rdfs:range rdf:resource="http://www.omg.org/spec/EDMC-SR/FND/Agreements/Contracts/ContractThirdParty"/>
   </owl:ObjectProperty>

   <owl:ObjectProperty rdf:about="http://www.edmcouncil.org/spec/EDMC-SR/FND/AgreementsExt/ContractElements/identifiesAs">
      <skos:definition>The business entity which is identified as a third party.</skos:definition>
      <rdfs:subPropertyOf rdf:resource="http://www.edmcouncil.org/spec/EDMC-SR/FND/AgreementsExt/ContractElements/IdentifiesContractPartyAs"/>
      <rdfs:domain rdf:resource="http://www.edmcouncil.org/spec/EDMC-SR/FND/AgreementsExt/ContractElements/ContractThirdPartyIdentification"/>
      <rdfs:range rdf:resource="http://www.omg.org/spec/EDMC-SR/BE/LegalEntities/FormalBusinessOrganizations/FormallyConstitutedOrganization"/>
   </owl:ObjectProperty>

   <owl:ObjectProperty rdf:about="http://www.edmcouncil.org/spec/EDMC-SR/FND/AgreementsExt/ContractElements/principalsIdentification">
      <skos:definition>The identification of the principals of the contract.</skos:definition>
      <rdfs:domain rdf:resource="http://www.omg.org/spec/EDMC-SR/FND/Agreements/Contracts/Contract"/>
      <rdfs:range rdf:resource="http://www.edmcouncil.org/spec/EDMC-SR/FND/AgreementsExt/ContractElements/ContractPartyIdentification"/>
   </owl:ObjectProperty>

   <owl:ObjectProperty rdf:about="http://www.edmcouncil.org/spec/EDMC-SR/FND/AgreementsExt/ContractElements/sectionContainsClause">
      <skos:definition>A clause contained in the contract section.</skos:definition>
      <rdfs:subPropertyOf rdf:resource="http://www.edmcouncil.org/spec/EDMC-SR/FND/AgreementsExt/ContractElements/writtenContractHasPart"/>
      <rdfs:domain rdf:resource="http://www.edmcouncil.org/spec/EDMC-SR/FND/AgreementsExt/ContractElements/ContractSection"/>
      <rdfs:range rdf:resource="http://www.edmcouncil.org/spec/EDMC-SR/FND/AgreementsExt/ContractElements/ContractClause"/>
   </owl:ObjectProperty>

   <owl:ObjectProperty rdf:about="http://www.edmcouncil.org/spec/EDMC-SR/FND/AgreementsExt/ContractElements/defines">
      <skos:definition>The definition of some matter as agreed by the parties to the contract and written in some part of that contract.</skos:definition>
      <rdfs:domain rdf:resource="http://www.omg.org/spec/EDMC-SR/FND/Agreements/Contracts/WrittenContract"/>
      <rdfs:range rdf:resource="http://www.omg.org/spec/EDMC-SR/FND/Agreements/Contracts/ContractualDefinition"/>
   </owl:ObjectProperty>

   <owl:ObjectProperty rdf:about="http://www.edmcouncil.org/spec/EDMC-SR/FND/AgreementsExt/ContractElements/definedInClause">
      <skos:definition>The individual clause of the contract in which the set of terms is defined, if applicable.</skos:definition>
      <rdfs:subPropertyOf rdf:resource="http://www.edmcouncil.org/spec/EDMC-SR/FND/AgreementsExt/ContractElements/definedInSection"/>
      <rdfs:domain rdf:resource="http://www.omg.org/spec/EDMC-SR/FND/Agreements/Contracts/ContractTermsSet"/>
      <rdfs:range rdf:resource="http://www.edmcouncil.org/spec/EDMC-SR/FND/AgreementsExt/ContractElements/ContractClause"/>
   </owl:ObjectProperty>

   <owl:ObjectProperty rdf:about="http://www.edmcouncil.org/spec/EDMC-SR/FND/AgreementsExt/ContractElements/definedInSection">
      <skos:definition>The section of the contract in which the contract terms set is defined.</skos:definition>
      <rdfs:domain rdf:resource="http://www.omg.org/spec/EDMC-SR/FND/Agreements/Contracts/ContractTermsSet"/>
      <rdfs:range rdf:resource="http://www.edmcouncil.org/spec/EDMC-SR/FND/AgreementsExt/ContractElements/ContractSection"/>
   </owl:ObjectProperty>

   <owl:ObjectProperty rdf:about="http://www.edmcouncil.org/spec/EDMC-SR/FND/AgreementsExt/ContractElements/identifiesContractPrincipalAs">
      <skos:definition>The business entities which are identified as the principals to the contract.</skos:definition>
      <rdfs:subPropertyOf rdf:resource="http://www.edmcouncil.org/spec/EDMC-SR/FND/AgreementsExt/ContractElements/IdentifiesContractPartyAs"/>
      <rdfs:domain rdf:resource="http://www.edmcouncil.org/spec/EDMC-SR/FND/AgreementsExt/ContractElements/ContractPrincipalsIdentification"/>
      <rdfs:range rdf:resource="http://www.omg.org/spec/EDMC-SR/BE/LegalEntities/LEIEntities/ContractuallyCapableEntity"/>
   </owl:ObjectProperty>

   <owl:ObjectProperty rdf:about="http://www.edmcouncil.org/spec/EDMC-SR/FND/AgreementsExt/ContractElements/writtenContractHasPart">
      <skos:definition>A formal part of the contract such as a clause or term.</skos:definition>
      <rdfs:subPropertyOf rdf:resource="http://www.edmcouncil.org/spec/EDMC-SR/FND/Information/InfoCore/hasPart"/>
      <rdfs:domain rdf:resource="http://www.omg.org/spec/EDMC-SR/FND/Agreements/Contracts/WrittenContract"/>
      <rdfs:range rdf:resource="http://www.edmcouncil.org/spec/EDMC-SR/FND/AgreementsExt/ContractElements/ContractPart"/>
   </owl:ObjectProperty>

   <!--Data Properties-->

<!--Annotation Properties-->

<!--Classes-->

<owl:Class rdf:about="http://www.edmcouncil.org/spec/EDMC-SR/FND/AgreementsExt/ContractElements/ContractClause">
      <rdfs:label>Contract Clause</rdfs:label>
      <skos:definition>A set of contractual terms, grouped according to subject, intent or the type of rights and / or obligations to which it refers.</skos:definition>
      <rdfs:subClassOf rdf:resource="http://www.edmcouncil.org/spec/EDMC-SR/FND/AgreementsExt/ContractElements/ContractPart"/>
   </owl:Class>

   <owl:Class rdf:about="http://www.edmcouncil.org/spec/EDMC-SR/FND/AgreementsExt/ContractElements/ContractPart">
      <rdfs:label>Contract Part</rdfs:label>
      <skos:definition>A formal part of a contract such as a clause or term.</skos:definition>
      <rdfs:subClassOf rdf:resource="http://www.omg.org/spec/EDMC-SR/FND/Agreements/Contracts/ContractualElement"/>
      <rdfs:subClassOf rdf:resource="http://www.edmcouncil.org/spec/EDMC-SR/FND/Relative/Mereological/Part"/>
      <rdfs:subClassOf rdf:resource="http://www.edmcouncil.org/spec/EDMC-SR/FND/Information/InfoCore/WrittenInformation"/>
   </owl:Class>

   <owl:Class rdf:about="http://www.edmcouncil.org/spec/EDMC-SR/FND/AgreementsExt/ContractElements/ContractPartyIdentification">
      <rdfs:label>Contract Party Identification</rdfs:label>
      <skos:definition>The identification of parties to a contract. This is usually but not necessarily identified in the preamble to a contract.</skos:definition>
      <rdfs:subClassOf rdf:resource="http://www.edmcouncil.org/spec/EDMC-SR/FND/Information/Identification/PartyIdentification"/>
   </owl:Class>

   <owl:Class rdf:about="http://www.edmcouncil.org/spec/EDMC-SR/FND/AgreementsExt/ContractElements/ContractPreamble">
      <rdfs:label>Contract Preamble</rdfs:label>
      <skos:definition>The part of a contract which defines the parties and gives sufficient information for them to be unambiguously identified, along with other pertinent information such as the subject of the contract.</skos:definition>
   </owl:Class>

   <owl:Class rdf:about="http://www.edmcouncil.org/spec/EDMC-SR/FND/AgreementsExt/ContractElements/ContractPrincipalsIdentification">
      <rdfs:label>Contract Principals Identification</rdfs:label>
      <skos:definition>The identification of the principals to a contract.</skos:definition>
      <rdfs:subClassOf rdf:resource="http://www.edmcouncil.org/spec/EDMC-SR/FND/AgreementsExt/ContractElements/ContractPartyIdentification"/>
   </owl:Class>

   <owl:Class rdf:about="http://www.edmcouncil.org/spec/EDMC-SR/FND/AgreementsExt/ContractElements/ContractSection">
      <rdfs:label>Contract Section</rdfs:label>
      <skos:definition>A formally identified Section of a Contract, comtaining terms dealing with a specific type of subject matter.</skos:definition>
   </owl:Class>

   <owl:Class rdf:about="http://www.edmcouncil.org/spec/EDMC-SR/FND/AgreementsExt/ContractElements/ContractTerm">
      <rdfs:label>Contract Term</rdfs:label>
      <skos:definition>An individual term in a Contract. Forms part of a set of Contractual Terms. Also exists within a Clause of a Contract A Clause exists within a Section of a Contract</skos:definition>
   </owl:Class>

   <owl:Class rdf:about="http://www.edmcouncil.org/spec/EDMC-SR/FND/AgreementsExt/ContractElements/ContractThirdPartyIdentification">
      <rdfs:label>Contract Third Party Identification</rdfs:label>
      <skos:definition>The identification of any third parties referred to in a contract but not being signatories to that contract. This would for example be the identification of calculation agents in a derivatives contract.</skos:definition>
   </owl:Class>

   <owl:Class rdf:about="http://www.edmcouncil.org/spec/EDMC-SR/FND/AgreementsExt/ContractElements/RepresentationsSection">
      <rdfs:label>Representations Section</rdfs:label>
      <skos:definition>Section containing statements held out by one party to the other as being true and correct at the time of the Agreement. A representation, as contained in this section of a contract, is a statement by one other party asserting that some given state of the world exists.</skos:definition>
      <skos:editorialNote>This is the contract section which formalizes these aspects of the Agreement between the parties. Things still to tease out: there is a difference at law between a warranty and a representation. There are differences between the implications if one or other proves to be untrue: one will render the contract void; the other renders only specific elements of the contract void or makes some difference between those elements. A warranty is likely a stronger assertion thatn a representation (has greater impact).</skos:editorialNote>
   </owl:Class>

   <owl:Class rdf:about="http://www.edmcouncil.org/spec/EDMC-SR/FND/AgreementsExt/ContractElements/WarrantiesSection">
      <rdfs:label>Warranties Section</rdfs:label>
      <skos:definition>Section defining what is warranted by either party to the other. A warranty, as contained in this section of a contract, is a statement by one other party asserting that some given state of the world exists.</skos:definition>
      <skos:editorialNote>This is the contract section which formalizes these aspects of the Agreement between the parties. Things still to tease out: there is a difference at law between a warranty and a representation. There are differences between the implications if one or other proves to be untrue: one will render the contract void; the other renders only specific elements of the contract void or makes some difference between those elements. A warranty is likely a stronger assertion thatn a representation (has greater impact).</skos:editorialNote>
   </owl:Class>

   <owl:Class rdf:about="http://www.edmcouncil.org/spec/EDMC-SR/FND/AgreementsExt/ContractElements/DRIP">
      <rdfs:label>DRIP</rdfs:label>
      <skos:definition>A kind of financial contract.</skos:definition>
      <skos:editorialNote>This term is awaitilng further analysis and will then be moved to the appropriate financial instrument section.</skos:editorialNote>
      <rdfs:subClassOf rdf:resource="http://www.omg.org/spec/EDMC-SR/FND/Agreements/Contracts/BilateralContract"/>
   </owl:Class>

   <!--Individuals-->

</rdf:RDF>