<?xml version="1.0" encoding="UTF-8"?>
<rdf:RDF xmlns:xsd="http://www.w3.org/2001/XMLSchema#"
         xmlns:sm="http://www.omg.org/techprocess/ab/SpecificationMetadata/"
         xmlns:fibo-fnd-utl-av="http://www.omg.org/spec/EDMC-FIBO/FND/Utilities/AnnotationVocabulary/"
         xmlns:rdf="http://www.w3.org/1999/02/22-rdf-syntax-ns#"
         xmlns:rdfs="http://www.w3.org/2000/01/rdf-schema#"
         xmlns:owl="http://www.w3.org/2002/07/owl#"
         xmlns:skos="http://www.w3.org/2004/02/skos/core#"
         xmlns:dc="http://purl.org/dc/terms/"
         xml:base="http://www.edmcouncil.org/spec/EDMC-SR/FND/AgreementsExt/ContractsExtensions/">

   <owl:Ontology rdf:about="http://www.edmcouncil.org/spec/EDMC-SR/FND/AgreementsExt/ContractsExtensions/">
      <owl:imports rdf:resource="http://www.omg.org/spec/EDMC-SR/BE/LegalEntities/LEIEntities/"/>
      <owl:imports rdf:resource="http://www.omg.org/spec/EDMC-SR/FND/Agreements/Contracts/"/>
   </owl:Ontology>

   <!--Datatypes-->

<!--Object Properties-->

<owl:ObjectProperty rdf:about="http://www.edmcouncil.org/spec/EDMC-SR/FND/AgreementsExt/ContractsExtensions/contractCounterpartyIdentity">
      <skos:definition>The legal entity which is identified as the counterparty to the contract, and which would be entitled to any rights granted by the principal to the contract.</skos:definition>
      <rdfs:subPropertyOf rdf:resource="http://www.edmcouncil.org/spec/EDMC-SR/FND/AgreementsExt/ContractsExtensions/contractPartyIdentity"/>
      <rdfs:domain rdf:resource="http://www.omg.org/spec/EDMC-SR/FND/Agreements/Contracts/ContractCounterparty"/>
      <rdfs:range rdf:resource="http://www.omg.org/spec/EDMC-SR/BE/LegalEntities/LEIEntities/ContractuallyCapableEntity"/>
   </owl:ObjectProperty>

   <owl:ObjectProperty rdf:about="http://www.edmcouncil.org/spec/EDMC-SR/FND/AgreementsExt/ContractsExtensions/contractPartyIdentity">
      <skos:definition>The legal entity which is identified as a party to the contract.</skos:definition>
      <skos:editorialNote>It is possible for a party to a contract to be a minor, and in so doing takes the rights but not the obligations to the contract.</skos:editorialNote>
      <rdfs:subPropertyOf rdf:resource="http://www.omg.org/spec/EDMC-SR/FND/Parties/Parties/partyInRoleHasIdentity"/>
      <rdfs:domain rdf:resource="http://www.edmcouncil.org/spec/EDMC-SR/FND/AgreementsExt/ContractsExtensions/ContractParty"/>
      <rdfs:range rdf:resource="http://www.omg.org/spec/EDMC-SR/BE/LegalEntities/LEIEntities/ContractuallyCapableEntity"/>
   </owl:ObjectProperty>

   <owl:ObjectProperty rdf:about="http://www.edmcouncil.org/spec/EDMC-SR/FND/AgreementsExt/ContractsExtensions/contractPrincipalIdentity">
      <skos:definition>The legal entity which is identified as the principal of the contract.</skos:definition>
      <skos:editorialNote>This is usually identified as such in the formal preamble to the contract if there is one. It may also be the issuer of a security.</skos:editorialNote>
      <rdfs:subPropertyOf rdf:resource="http://www.edmcouncil.org/spec/EDMC-SR/FND/AgreementsExt/ContractsExtensions/contractPartyIdentity"/>
      <rdfs:domain rdf:resource="http://www.omg.org/spec/EDMC-SR/FND/Agreements/Contracts/ContractPrincipal"/>
      <rdfs:range rdf:resource="http://www.omg.org/spec/EDMC-SR/BE/LegalEntities/LEIEntities/ContractuallyCapableEntity"/>
   </owl:ObjectProperty>

   <owl:ObjectProperty rdf:about="http://www.edmcouncil.org/spec/EDMC-SR/FND/AgreementsExt/ContractsExtensions/embodies">
      <skos:definition>A relationship between two parties, embodied in and created by that contract.</skos:definition>
      <rdfs:domain rdf:resource="http://www.omg.org/spec/EDMC-SR/FND/Agreements/Contracts/Contract"/>
      <rdfs:range rdf:resource="http://www.omg.org/spec/EDMC-SR/FND/Agreements/Contracts/ContractualRelationship"/>
   </owl:ObjectProperty>

   <owl:ObjectProperty rdf:about="http://www.edmcouncil.org/spec/EDMC-SR/FND/AgreementsExt/ContractsExtensions/hasParty">
      <skos:definition>A party to the contract, that is one of the signatories. This is a legal entity which is a signatory to or holder of the contract, and which grants or concedes certain rights and obligations as defined in the contract.</skos:definition>
      <rdfs:subPropertyOf rdf:resource="http://www.omg.org/spec/EDMC-SR/FND/Parties/Parties/hasPartyInRole"/>
      <rdfs:domain rdf:resource="http://www.omg.org/spec/EDMC-SR/FND/Agreements/Contracts/Contract"/>
      <rdfs:range rdf:resource="http://www.edmcouncil.org/spec/EDMC-SR/FND/AgreementsExt/ContractsExtensions/ContractParty"/>
   </owl:ObjectProperty>

   <owl:ObjectProperty rdf:about="http://www.edmcouncil.org/spec/EDMC-SR/FND/AgreementsExt/ContractsExtensions/hasProvisions">
      <skos:definition>Termination provisions as contained in the Contract. These set out the conditions under which the contract may be terminated and the rights and obligations of each party in the event of such termination.</skos:definition>
      <rdfs:subPropertyOf rdf:resource="http://www.omg.org/spec/EDMC-SR/FND/Agreements/Contracts/contractHasTerms"/>
      <rdfs:domain rdf:resource="http://www.omg.org/spec/EDMC-SR/FND/Agreements/Contracts/WrittenContract"/>
      <rdfs:range rdf:resource="http://www.edmcouncil.org/spec/EDMC-SR/FND/AgreementsExt/ContractsExtensions/TerminationProvisions"/>
   </owl:ObjectProperty>

   <!--Data Properties-->

<!--Annotation Properties-->

<!--Classes-->

<owl:Class rdf:about="http://www.edmcouncil.org/spec/EDMC-SR/FND/AgreementsExt/ContractsExtensions/ContractParty">
      <rdfs:label>Contract Party</rdfs:label>
      <skos:definition>A Party to some Contract.</skos:definition>
      <rdfs:subClassOf rdf:resource="http://www.edmcouncil.org/spec/EDMC-SR/FND/AgreementsExt/AgreementsInverses/AgreementParty"/>
      <rdfs:subClassOf rdf:resource="http://www.omg.org/spec/EDMC-SR/FND/Parties/Parties/PartyInRole"/>
   </owl:Class>

   <owl:Class rdf:about="http://www.edmcouncil.org/spec/EDMC-SR/FND/AgreementsExt/ContractsExtensions/TerminationProvisions">
      <rdfs:label>Termination Provisions</rdfs:label>
      <skos:definition>Formal terms setting out how the written contract may be terminated and what happens when it is.</skos:definition>
      <rdfs:subClassOf rdf:resource="http://www.omg.org/spec/EDMC-SR/FND/Agreements/Contracts/ContractTermsSet"/>
   </owl:Class>

   <!--Individuals-->

</rdf:RDF>