<?xml version="1.0" encoding="UTF-8"?>
<rdf:RDF xmlns:xsd="http://www.w3.org/2001/XMLSchema#"
         xmlns:sm="http://www.omg.org/techprocess/ab/SpecificationMetadata/"
         xmlns:fibo-fnd-utl-av="http://www.omg.org/spec/EDMC-FIBO/FND/Utilities/AnnotationVocabulary/"
         xmlns:rdf="http://www.w3.org/1999/02/22-rdf-syntax-ns#"
         xmlns:rdfs="http://www.w3.org/2000/01/rdf-schema#"
         xmlns:owl="http://www.w3.org/2002/07/owl#"
         xmlns:skos="http://www.w3.org/2004/02/skos/core#"
         xmlns:dc="http://purl.org/dc/terms/"
         xml:base="http://www.omg.org/spec/EDMC-SR/FND/Law/LegalCore/">

   <owl:Ontology rdf:about="http://www.omg.org/spec/EDMC-SR/FND/Law/LegalCore/">
      <owl:imports rdf:resource="http://www.edmcouncil.org/spec/EDMC-SR/UO/Lattice/"/>
   </owl:Ontology>

   <!--Datatypes-->

<!--Object Properties-->

<owl:ObjectProperty rdf:about="http://www.omg.org/spec/EDMC-SR/FND/Law/LegalCore/governs">
      <skos:definition>The constitution governs and constrains the application of the or each body of law in the jurisdiction other framework to which it applies.</skos:definition>
      <skos:editorialNote>These relations are also general to non national equivalents where for example the constitution is the company articles and the law is the bylaws of the company.</skos:editorialNote>
      <rdfs:subPropertyOf rdf:resource="http://www.omg.org/spec/EDMC-SR/FND/Relations/Relations/governs"/>
      <rdfs:domain rdf:resource="http://www.omg.org/spec/EDMC-SR/FND/Law/LegalCore/Constitution"/>
      <rdfs:range rdf:resource="http://www.omg.org/spec/EDMC-SR/FND/Law/LegalCore/Law"/>
   </owl:ObjectProperty>

   <!--Data Properties-->

<!--Annotation Properties-->

<!--Classes-->

<owl:Class rdf:about="http://www.omg.org/spec/EDMC-SR/FND/Law/LegalCore/Constitution">
      <rdfs:label>Constitution</rdfs:label>
      <rdfs:subClassOf rdf:resource="http://www.edmcouncil.org/spec/EDMC-SR/UO/Lattice/Concrete"/>
      <rdfs:subClassOf rdf:resource="http://www.edmcouncil.org/spec/EDMC-SR/UO/OntologicalDegree/IndependentThing"/>
      <rdfs:subClassOf rdf:resource="http://www.edmcouncil.org/spec/EDMC-SR/UO/Lattice/ContinuantThing"/>
   </owl:Class>

   <owl:Class rdf:about="http://www.omg.org/spec/EDMC-SR/FND/Law/LegalCore/CourtOfLaw">
      <rdfs:label>Court Of Law</rdfs:label>
      <skos:definition>Some formal body with the mandate to hear disputes or cases.</skos:definition>
      <skos:editorialNote>temporary definition.</skos:editorialNote>
      <rdfs:subClassOf rdf:resource="http://www.omg.org/spec/EDMC-SR/FND/Organizations/FormalOrganizations/FormalOrganization"/>
   </owl:Class>

   <owl:Class rdf:about="http://www.omg.org/spec/EDMC-SR/FND/Law/LegalCore/GovernmentalConstitution">
      <rdfs:label>Governmental Constitution</rdfs:label>
      <skos:definition>A body of rules, commitments and statements that set out how a country, state or territory is to be run.</skos:definition>
      <skos:editorialNote>This defines the framework in which laws are made and in which they have force.</skos:editorialNote>
      <rdfs:subClassOf rdf:resource="http://www.omg.org/spec/EDMC-SR/FND/Law/LegalCore/Constitution"/>
   </owl:Class>

   <owl:Class rdf:about="http://www.omg.org/spec/EDMC-SR/FND/Law/LegalCore/Law">
      <rdfs:label>Law</rdfs:label>
   </owl:Class>

   <owl:Class rdf:about="http://www.omg.org/spec/EDMC-SR/FND/Law/LegalCore/Ordinance">
      <rdfs:label>Ordinance</rdfs:label>
      <skos:definition>An authoritative rule or law; a decree or command; a public injunction or regulation, such as a city ordinance against excessive horn blowing. (Source: Dictionary.com)</skos:definition>
      <rdfs:subClassOf rdf:resource="http://www.omg.org/spec/EDMC-SR/FND/Law/LegalCore/Law"/>
   </owl:Class>

   <!--Individuals-->

</rdf:RDF>