<?xml version="1.0" encoding="UTF-8"?>
  
<!DOCTYPE rdf:RDF [
    <!ENTITY fibo-be-oac-cpty "http://spec.edmcouncil.org/fibo/red/be/ownership-and-control/control-parties/">
    <!ENTITY fibo-fnd-pty-pty "http://spec.edmcouncil.org/fibo/red/fnd/parties/parties/">
    <!ENTITY fibo-fnd-org-fm "http://spec.edmcouncil.org/fibo/red/fnd/organizations/formal-organizations/">
    <!ENTITY fibo-fnd-oac-ctl "http://spec.edmcouncil.org/fibo/red/fnd/ownership-and-control/control/">
    <!ENTITY fibo-be-oac-opty "http://spec.edmcouncil.org/fibo/red/be/ownership-and-control/ownership-parties/">
    <!ENTITY fibo-fnd-utl-bt "http://spec.edmcouncil.org/fibo/red/fnd/utilities/business-facing-types/">
    <!ENTITY fibo-fnd-law-lcap "http://spec.edmcouncil.org/fibo/red/fnd/law/legal-capacities/">
    <!ENTITY fibo-fnd-agr-ctr "http://spec.edmcouncil.org/fibo/red/fnd/agreements/contracts/">
    <!ENTITY fibo-fnd-law-cor "http://spec.edmcouncil.org/fibo/red/fnd/law/legal-core/">
    <!ENTITY fibo-be-le-fbo "http://spec.edmcouncil.org/fibo/red/be/legal-entities/formal-business-organizations/">
    <!ENTITY fibo-be-oacx-cptyx "http://spec.edmcouncil.org/fibo/red/be/ownership-control-ext/control-parties-extras/">
    <!ENTITY fibo-fnd-rel-rel "http://spec.edmcouncil.org/fibo/red/fnd/relations/relations/">
    <!ENTITY fibo-fnd-aap-agt "http://spec.edmcouncil.org/fibo/red/fnd/agents-and-people/agents/">
]>

<rdf:RDF xmlns:xsd="http://www.w3.org/2001/XMLSchema#"
         xmlns:sm="http://www.omg.org/techprocess/ab/SpecificationMetadata/"
         xmlns:xs="http://www.w3.org/2001/XMLSchema"
         xmlns:fibo-fnd-utl-av="http://www.omg.org/spec/EDMC-FIBO/FND/Utilities/AnnotationVocabulary/"
         xmlns:rdf="http://www.w3.org/1999/02/22-rdf-syntax-ns#"
         xmlns:rdfs="http://www.w3.org/2000/01/rdf-schema#"
         xmlns:owl="http://www.w3.org/2002/07/owl#"
         xmlns:skos="http://www.w3.org/2004/02/skos/core#"
         xmlns:dc="http://purl.org/dc/terms/"
         xml:base="http://spec.edmcouncil.org/fibo/red/be/ownership-and-control/control-parties/">

   <owl:Ontology rdf:about="http://spec.edmcouncil.org/fibo/red/be/ownership-and-control/control-parties/">
      <owl:imports rdf:resource="http://spec.edmcouncil.org/fibo/red/fnd/parties/parties/"/>
      <owl:imports rdf:resource="http://spec.edmcouncil.org/fibo/red/fnd/organizations/formal-organizations/"/>
      <owl:imports rdf:resource="http://spec.edmcouncil.org/fibo/red/fnd/ownership-and-control/control/"/>
      <owl:imports rdf:resource="http://spec.edmcouncil.org/fibo/red/be/ownership-and-control/ownership-parties/"/>
      <owl:imports rdf:resource="http://spec.edmcouncil.org/fibo/red/fnd/utilities/business-facing-types/"/>
      <owl:imports rdf:resource="http://spec.edmcouncil.org/fibo/red/fnd/law/legal-capacities/"/>
      <owl:imports rdf:resource="http://spec.edmcouncil.org/fibo/red/fnd/agreements/contracts/"/>
      <owl:imports rdf:resource="http://spec.edmcouncil.org/fibo/red/fnd/law/legal-core/"/>
      <owl:imports rdf:resource="http://spec.edmcouncil.org/fibo/red/be/legal-entities/formal-business-organizations/"/>
      <owl:imports rdf:resource="http://spec.edmcouncil.org/fibo/red/be/ownership-control-ext/control-parties-extras/"/>
      <owl:imports rdf:resource="http://spec.edmcouncil.org/fibo/red/fnd/relations/relations/"/>
      <owl:imports rdf:resource="http://spec.edmcouncil.org/fibo/red/fnd/agents-and-people/agents/"/>
   </owl:Ontology>


  <!--
    ///////////////////////////////////////////////////////////////////////////////////////
    //
    // Datatypes
    //
    ///////////////////////////////////////////////////////////////////////////////////////
    -->



  <!--
    ///////////////////////////////////////////////////////////////////////////////////////
    //
    // Object Properties
    //
    ///////////////////////////////////////////////////////////////////////////////////////
    -->


<owl:ObjectProperty rdf:about="&fibo-be-oac-cpty;constitutionalContractualControlIsConferredBy">
      <rdfs:label>constitutional contractual control is conferred by</rdfs:label>
      <skos:definition>The control is conferred on the party by means of the formal covering agreement by which the organization is constituted, that is the agreement between the principals of the organization.</skos:definition>
      <rdfs:subPropertyOf rdf:resource="&fibo-be-oac-cpty;contractualControlIsConferredBy"/>
      <rdfs:domain rdf:resource="&fibo-be-oac-cpty;ConstitutionalContractualControl"/>
      <rdfs:range rdf:resource="&fibo-be-le-fbo;OrganizationCoveringAgreement"/>
   </owl:ObjectProperty>

   <owl:ObjectProperty rdf:about="&fibo-be-oac-cpty;contractualControlIsConferredBy">
      <rdfs:label>contractual control is conferred by</rdfs:label>
      <skos:definition>The control is conferred on the party by means of some contract.</skos:definition>
      <rdfs:subPropertyOf rdf:resource="&fibo-fnd-law-lcap;isConferredBy"/>
      <rdfs:domain rdf:resource="&fibo-be-oac-cpty;ContractualControl"/>
      <rdfs:range rdf:resource="&fibo-fnd-agr-ctr;Contract"/>
   </owl:ObjectProperty>

   <owl:ObjectProperty rdf:about="&fibo-be-oac-cpty;controlledPartyIsControlledToSomeDegreeBy">
      <rdfs:label>controlled party is controlled to some degree by</rdfs:label>
      <rdfs:subPropertyOf rdf:resource="&fibo-be-oac-cpty;isControlledToSomeDegreeBy"/>
      <rdfs:domain rdf:resource="&fibo-be-oac-cpty;ControlledParty"/>
      <rdfs:range rdf:resource="&fibo-fnd-aap-agt;AutonomousAgent"/>
   </owl:ObjectProperty>

   <owl:ObjectProperty rdf:about="&fibo-be-oac-cpty;courtAppoinredControlIsConferredBy">
      <rdfs:label>court appoinred control is conferred by</rdfs:label>
      <skos:definition>The control which is vested in the controlling party is conferred upon that party through some court of law.</skos:definition>
      <rdfs:subPropertyOf rdf:resource="&fibo-fnd-law-lcap;isConferredBy"/>
      <rdfs:domain rdf:resource="&fibo-be-oac-cpty;CourtAppointedControl"/>
      <rdfs:range rdf:resource="&fibo-fnd-law-cor;CourtOfLaw"/>
   </owl:ObjectProperty>

   <owl:ObjectProperty rdf:about="&fibo-be-oac-cpty;jointControllingPartyIdentity">
      <rdfs:label>joint controlling party identity</rdfs:label>
      <skos:definition>The identity of the Party is some group of entities which have formed some alliance or agreement in terms of which they jointly exercise control over the controlled organization.</skos:definition>
      <rdfs:subPropertyOf rdf:resource="&fibo-fnd-pty-pty;hasIdentity"/>
      <rdfs:domain rdf:resource="&fibo-be-oac-cpty;JointControllingParty"/>
      <rdfs:range rdf:resource="&fibo-be-oac-cpty;ControllingAlliance"/>
   </owl:ObjectProperty>

   <owl:ObjectProperty rdf:about="&fibo-be-oac-cpty;limitedControllingPartyHasNatureOControl">
      <rdfs:label>limited controlling party has nature o control</rdfs:label>
      <skos:definition>The type of control for which the party has the stated percentage.</skos:definition>
      <rdfs:subPropertyOf rdf:resource="&fibo-be-oac-cpty;exercisesSomeDegreeOf"/>
      <rdfs:domain rdf:resource="&fibo-be-oac-cpty;LimitedControllingParty"/>
      <rdfs:range rdf:resource="&fibo-be-oac-cpty;LimitedDeFactoControl"/>
   </owl:ObjectProperty>

   <owl:ObjectProperty rdf:about="&fibo-be-oac-cpty;exercisesContractualControl">
      <rdfs:label>exercises contractual control</rdfs:label>
      <skos:definition>Control is exercised by the party, which is conferred by some contractual agreement.</skos:definition>
      <rdfs:subPropertyOf rdf:resource="&fibo-be-oac-cpty;holdsSomeInstrumentOfDeJureControl"/>
      <rdfs:domain rdf:resource="&fibo-be-oac-cpty;ContractualControllingParty"/>
      <rdfs:range rdf:resource="&fibo-be-oac-cpty;ContractualControl"/>
   </owl:ObjectProperty>

   <owl:ObjectProperty rdf:about="&fibo-be-oac-cpty;exercisesCourtAppointedControl">
      <rdfs:label>exercises court appointed control</rdfs:label>
      <skos:definition>Legal control exercised by the party, which is appointed by some court.</skos:definition>
      <rdfs:subPropertyOf rdf:resource="&fibo-be-oac-cpty;holdsSomeInstrumentOfDeJureControl"/>
      <rdfs:domain rdf:resource="&fibo-be-oac-cpty;Receiver"/>
      <rdfs:range rdf:resource="&fibo-be-oac-cpty;CourtAppointedControl"/>
   </owl:ObjectProperty>

   <owl:ObjectProperty rdf:about="&fibo-be-oac-cpty;exercisesInvestmentBasedDeFactoControl">
      <rdfs:label>exercises investment based de facto control</rdfs:label>
      <skos:definition>The party exercises some degree of de facto control based on some investment which they hold in the entity.</skos:definition>
      <rdfs:subPropertyOf rdf:resource="&fibo-be-oac-cpty;holdsSomeMeansOfDeFactoControl"/>
      <rdfs:domain rdf:resource="&fibo-be-oac-cpty;InvestmentBasedDeFactoControllingInterestParty"/>
      <rdfs:range rdf:resource="&fibo-be-oac-cpty;InvestmentBasedDeFactoControl"/>
   </owl:ObjectProperty>

   <owl:ObjectProperty rdf:about="&fibo-be-oac-cpty;hasSignificantControllingInterstParty">
      <rdfs:label>has significant controlling interst party</rdfs:label>
      <skos:definition>Some entity which owns a significant part of this company but not 50% or more.</skos:definition>
      <rdfs:subPropertyOf rdf:resource="&fibo-be-oac-cpty;hasControllingInterestParty"/>
      <rdfs:subPropertyOf rdf:resource="&fibo-be-oacx-cptyx;hasDeJureControllingInterestParty"/>
      <rdfs:domain rdf:resource="&fibo-be-le-fbo;FormallyConstitutedOrganization"/>
      <rdfs:range rdf:resource="&fibo-be-oac-cpty;SignificantControllingInterestParty"/>
   </owl:ObjectProperty>

   <owl:ObjectProperty rdf:about="&fibo-be-oac-cpty;hasTotalOwner">
      <rdfs:label>has total owner</rdfs:label>
      <skos:definition>The Formal Organization is totally owned and therefore wholly controlled by some party having 100% ownership in it.</skos:definition>
      <rdfs:subPropertyOf rdf:resource="&fibo-be-oac-opty;hasConstitutionalOwner"/>
      <rdfs:domain rdf:resource="&fibo-be-le-fbo;FormallyConstitutedOrganization"/>
      <rdfs:range rdf:resource="&fibo-be-oac-cpty;TotalOwner"/>
   </owl:ObjectProperty>

   <owl:ObjectProperty rdf:about="&fibo-be-oac-cpty;hasControllingInterestParty">
      <rdfs:label>has controlling interest party</rdfs:label>
      <skos:definition>The Formal Organization is controlled in some way by some controlling party, that is some entity which exercises such control.</skos:definition>
      <rdfs:subPropertyOf rdf:resource="&fibo-fnd-pty-pty;hasPartyInRole"/>
      <rdfs:domain rdf:resource="&fibo-be-le-fbo;FormallyConstitutedOrganization"/>
      <rdfs:range rdf:resource="&fibo-be-oac-cpty;ControllingInterestParty"/>
   </owl:ObjectProperty>

   <owl:ObjectProperty rdf:about="&fibo-be-oac-cpty;hasDegreeOfControl">
      <rdfs:label>has degree of control</rdfs:label>
      <skos:definition>has degree of control, (partial, majority, or complete) either alone or with other parties, with respect to some activity</skos:definition>
      <rdfs:domain rdf:resource="&fibo-be-oac-cpty;EntityControllingParty"/>
      <rdfs:range rdf:resource="&fibo-be-oac-cpty;DegreeOfControl"/>
   </owl:ObjectProperty>

   <owl:ObjectProperty rdf:about="&fibo-be-oac-cpty;hasMajorityControllingParty">
      <rdfs:label>has majority controlling party</rdfs:label>
      <skos:definition>The parent of the company, if there is one.</skos:definition>
      <rdfs:subPropertyOf rdf:resource="&fibo-be-oac-cpty;isControlledToSomeDegreeBy"/>
      <rdfs:domain rdf:resource="&fibo-be-le-fbo;FormallyConstitutedOrganization"/>
      <rdfs:range rdf:resource="&fibo-be-oac-cpty;MajorityControllingParty"/>
   </owl:ObjectProperty>

   <owl:ObjectProperty rdf:about="&fibo-be-oac-cpty;exercisesSomeDegreeOf">
      <rdfs:label>exercises some degree of</rdfs:label>
      <skos:definition>has nature or kind of control, de facto or limited de facto control</skos:definition>
      <rdfs:domain rdf:resource="&fibo-be-oac-cpty;EntityControllingParty"/>
      <rdfs:range rdf:resource="&fibo-fnd-oac-ctl;DeFactoControl"/>
   </owl:ObjectProperty>

   <owl:ObjectProperty rdf:about="&fibo-be-oac-cpty;exercisesSomeInvestmentBasedDeFactoControl">
      <rdfs:label>exercises some investment based de facto control</rdfs:label>
      <skos:definition>The party exercises some de facto control based on some investment in equity.</skos:definition>
      <rdfs:subPropertyOf rdf:resource="&fibo-be-oac-cpty;holdsSomeMeansOfDeFactoControl"/>
      <rdfs:domain rdf:resource="&fibo-be-oac-cpty;ControllingLeverageParty"/>
      <rdfs:range rdf:resource="&fibo-be-oac-cpty;InvestmentBasedDeFactoControl"/>
   </owl:ObjectProperty>

   <owl:ObjectProperty rdf:about="&fibo-be-oac-cpty;holdsSomeInstrumentOfDeJureControl">
      <rdfs:label>holds some instrument of de jure control</rdfs:label>
      <skos:definition>Legal or contractually based control exercised by the party.</skos:definition>
      <rdfs:subPropertyOf rdf:resource="&fibo-be-oac-cpty;holdsSomeMeansOf"/>
      <rdfs:domain rdf:resource="&fibo-be-oac-cpty;DeJureControllingInterestParty"/>
      <rdfs:range rdf:resource="&fibo-be-oac-cpty;DeJureControllingInterest"/>
   </owl:ObjectProperty>

   <owl:ObjectProperty rdf:about="&fibo-be-oac-cpty;holdsSomeMeansOfDeFactoControl">
      <rdfs:label>holds some means of de facto control</rdfs:label>
      <skos:definition>The party exercises some control which is not based in law or contract but in some other means.</skos:definition>
      <rdfs:subPropertyOf rdf:resource="&fibo-be-oac-cpty;holdsSomeMeansOf"/>
      <rdfs:domain rdf:resource="&fibo-be-oac-cpty;DeFactoControllingInterestParty"/>
      <rdfs:range rdf:resource="&fibo-fnd-oac-ctl;DeFactoControl"/>
   </owl:ObjectProperty>

   <owl:ObjectProperty rdf:about="&fibo-be-oac-cpty;exercisesSomeInfluenceBasedDeFactoControl">
      <rdfs:label>exercises some influence based de facto control</rdfs:label>
      <skos:definition>Exercises some influence and control other than by means of investment.</skos:definition>
      <rdfs:subPropertyOf rdf:resource="&fibo-be-oac-cpty;holdsSomeMeansOfDeFactoControl"/>
      <rdfs:domain rdf:resource="&fibo-be-oac-cpty;InfluenceBasedDeFactoControllingParty"/>
      <rdfs:range rdf:resource="&fibo-be-oac-cpty;InfluenceBasedDeFactoControl"/>
   </owl:ObjectProperty>

   <owl:ObjectProperty rdf:about="&fibo-be-oac-cpty;holdsTheOptionToExercise">
      <rdfs:label>holds the option to exercise</rdfs:label>
      <skos:definition>Control which may optionally be exercised by the party.</skos:definition>
      <rdfs:subPropertyOf rdf:resource="&fibo-be-oac-cpty;holdsSomeMeansOf"/>
      <rdfs:domain rdf:resource="&fibo-be-oac-cpty;PartyHoldingSomeOptionForControl"/>
      <rdfs:range rdf:resource="&fibo-be-oac-cpty;DeJureControllingInterest"/>
   </owl:ObjectProperty>

   <owl:ObjectProperty rdf:about="&fibo-be-oac-cpty;holdsSomeMeansOf">
      <rdfs:label>holds some means of</rdfs:label>
      <skos:definition>Some means of control held by the party.</skos:definition>
      <rdfs:domain rdf:resource="&fibo-be-oac-cpty;ControllingInterestParty"/>
      <rdfs:range rdf:resource="&fibo-fnd-oac-ctl;Control"/>
   </owl:ObjectProperty>

   <owl:ObjectProperty rdf:about="&fibo-be-oac-cpty;basedOnInvestmentEquity">
      <rdfs:label>based on investment equity</rdfs:label>
      <skos:definition>Investment Based De Facto Control is based on the holding of some Investment Equity by some party.</skos:definition>
      <rdfs:subPropertyOf rdf:resource="&fibo-fnd-rel-rel;isConferredBy"/>
      <rdfs:domain rdf:resource="&fibo-be-oac-cpty;InvestmentBasedDeFactoControl"/>
      <rdfs:range rdf:resource="&fibo-be-oac-opty;InvestmentEquity"/>
   </owl:ObjectProperty>

   <owl:ObjectProperty rdf:about="&fibo-be-oac-cpty;isControlledToSomeDegreeBy">
      <rdfs:label>is controlled to some degree by</rdfs:label>
      <skos:definition>Some party which has some degree of control over the organization.</skos:definition>
      <rdfs:subPropertyOf rdf:resource="&fibo-fnd-rel-rel;isControlledBy"/>
      <rdfs:domain rdf:resource="&fibo-be-le-fbo;FormallyConstitutedOrganization"/>
      <rdfs:range rdf:resource="&fibo-be-oac-cpty;EntityControllingParty"/>
   </owl:ObjectProperty>


  <!--
    ///////////////////////////////////////////////////////////////////////////////////////
    //
    // Data Properties
    //
    ///////////////////////////////////////////////////////////////////////////////////////
    -->


<owl:DatatypeProperty rdf:about="&fibo-be-oac-cpty;percentageDeFactoControl">
      <rdfs:label>percentage de facto control</rdfs:label>
      <rdfs:range rdf:resource="&fibo-fnd-utl-bt;percentage"/>
   </owl:DatatypeProperty>

   <owl:DatatypeProperty rdf:about="&fibo-be-oac-cpty;percentageDeFactoControl.1">
      <rdfs:label>percentage de facto control</rdfs:label>
      <skos:definition>The percentage of control which the party is deemed or calculated as being able to exercise over the controlled entity.</skos:definition>
      <rdfs:range rdf:resource="&fibo-fnd-utl-bt;percentage"/>
   </owl:DatatypeProperty>


  <!--
    ///////////////////////////////////////////////////////////////////////////////////////
    //
    // Annotation Properties
    //
    ///////////////////////////////////////////////////////////////////////////////////////
    -->



  <!--
    ///////////////////////////////////////////////////////////////////////////////////////
    //
    // Classes
    //
    ///////////////////////////////////////////////////////////////////////////////////////
    -->


<owl:Class rdf:about="&fibo-be-oac-cpty;COCOBondholder">
      <rdfs:label>c o c o bondholder</rdfs:label>
      <skos:definition>Holder of bank bonds which convert to equity holdings in a bank.</skos:definition>
      <rdfs:subClassOf rdf:resource="&fibo-be-oac-cpty;PartyHoldingSomeOptionForControl"/>
   </owl:Class>

   <owl:Class rdf:about="&fibo-be-oac-cpty;ConstitutionalContractualControl">
      <rdfs:label>constitutional contractual control</rdfs:label>
      <skos:definition>Some control set out in some contract among the principals of an organization.</skos:definition>
      <rdfs:subClassOf rdf:resource="&fibo-be-oac-cpty;ContractualControl"/>
      <rdfs:subClassOf rdf:resource="&fibo-be-oac-cpty;ConstitutionalDeJureControl"/>
   </owl:Class>

   <owl:Class rdf:about="&fibo-be-oac-cpty;ConstitutionalDeJureControl">
      <rdfs:label>constitutional de jure control</rdfs:label>
      <skos:definition>Control which is based in some instrument which has constitutional standing (is constitutive of the entity) such as voting shares, general partner equity etc.</skos:definition>
      <rdfs:subClassOf rdf:resource="&fibo-be-oac-cpty;DeJureControllingInterest"/>
   </owl:Class>

   <owl:Class rdf:about="&fibo-be-oac-cpty;ContractualControl">
      <rdfs:label>contractual control</rdfs:label>
      <skos:definition>Control vested in an entity by virtue of the terms in some contract between that entity and others.</skos:definition>
      <rdfs:subClassOf rdf:resource="&fibo-fnd-oac-ctl;DeJureControl"/>
   </owl:Class>

   <owl:Class rdf:about="&fibo-be-oac-cpty;ContractualControllingParty">
      <rdfs:label>contractual controlling party</rdfs:label>
      <skos:definition>A party which exercises some control which is set out in some contract.</skos:definition>
      <rdfs:subClassOf rdf:resource="&fibo-be-oac-cpty;DeJureControllingInterestParty"/>
   </owl:Class>

   <owl:Class rdf:about="&fibo-be-oac-cpty;ControlledParty">
      <rdfs:label>controlled party</rdfs:label>
      <skos:definition>Some party which is controlled in some way and to some degree by some other party.</skos:definition>
      <rdfs:subClassOf rdf:resource="&fibo-fnd-pty-pty;PartyInRole"/>
   </owl:Class>

   <owl:Class rdf:about="&fibo-be-oac-cpty;ControllingAlliance">
      <rdfs:label>controlling alliance</rdfs:label>
      <skos:definition>Some group of entities which have formed some alliance or agreement in terms of which they jointly exercise control over some entity.</skos:definition>
      <rdfs:subClassOf rdf:resource="&fibo-fnd-org-fm;Group"/>
   </owl:Class>

   <owl:Class rdf:about="&fibo-be-oac-cpty;ControllingInterestOptionHolder">
      <rdfs:label>controlling interest option holder</rdfs:label>
      <skos:definition>A party which holds some option which may be exercised to confer on that party some de jure controlling interest at some time in the future and at the discretion of that holder.</skos:definition>
   </owl:Class>

   <owl:Class rdf:about="&fibo-be-oac-cpty;ControllingInterestParty">
      <rdfs:label>controlling interest party</rdfs:label>
      <skos:definition>Some Party which holds some form of controlling interest in some other party in some context.</skos:definition>
      <rdfs:subClassOf rdf:resource="&fibo-fnd-oac-ctl;ControllingParty"/>
   </owl:Class>

   <owl:Class rdf:about="&fibo-be-oac-cpty;ControllingLeverageParty">
      <rdfs:label>controlling leverage party</rdfs:label>
      <skos:definition>A party which exercises control as a result of some investment in an equity.</skos:definition>
      <rdfs:subClassOf rdf:resource="&fibo-be-oac-cpty;DeFactoControllingInterestParty"/>
   </owl:Class>

   <owl:Class rdf:about="&fibo-be-oac-cpty;CourtAppointedControl">
      <rdfs:label>court appointed control</rdfs:label>
      <skos:definition>Control conferred on some entity by act of some court, for example in the context of receivership.</skos:definition>
   </owl:Class>

   <owl:Class rdf:about="&fibo-be-oac-cpty;DeFactoControllingInterestParty">
      <rdfs:label>de facto controlling interest party</rdfs:label>
      <rdfs:subClassOf rdf:resource="&fibo-be-oac-cpty;ControllingInterestParty"/>
   </owl:Class>

   <owl:Class rdf:about="&fibo-be-oac-cpty;DeJureControllingInterest">
      <rdfs:label>de jure controlling interest</rdfs:label>
      <skos:definition>Control which is formalized by some formal legal construct.</skos:definition>
   </owl:Class>

   <owl:Class rdf:about="&fibo-be-oac-cpty;DeJureControllingInterestParty">
      <rdfs:label>de jure controlling interest party</rdfs:label>
      <skos:definition>An entity which exercises de jure control.</skos:definition>
   </owl:Class>

   <owl:Class rdf:about="&fibo-be-oac-cpty;DegreeOfControl">
      <rdfs:label>degree of control</rdfs:label>
   </owl:Class>

   <owl:Class rdf:about="&fibo-be-oac-cpty;EntityControllingParty">
      <rdfs:label>entity controlling party</rdfs:label>
      <skos:definition>Some party which is able to direct the activities of some business entity.</skos:definition>
   </owl:Class>

   <owl:Class rdf:about="&fibo-be-oac-cpty;EquityBasedDeJureControl">
      <rdfs:label>equity based de jure control</rdfs:label>
      <skos:definition>De Jure controlling interest in an entity which is based on the holding of some form of equity in that entity.</skos:definition>
   </owl:Class>

   <owl:Class rdf:about="&fibo-be-oac-cpty;InfluenceBasedDeFactoControl">
      <rdfs:label>influence based de facto control</rdfs:label>
      <skos:definition>Some influence and control over some entity other than by means of investment in that entity.</skos:definition>
      <rdfs:subClassOf rdf:resource="&fibo-fnd-oac-ctl;DeFactoControl"/>
   </owl:Class>

   <owl:Class rdf:about="&fibo-be-oac-cpty;InfluenceBasedDeFactoControllingParty">
      <rdfs:label>influence based de facto controlling party</rdfs:label>
      <skos:definition>A party which exercises some influence and control over the entity other than by means of investment.</skos:definition>
   </owl:Class>

   <owl:Class rdf:about="&fibo-be-oac-cpty;InvestmentBasedDeFactoControl">
      <rdfs:label>investment based de facto control</rdfs:label>
      <skos:definition>Control which arises through some investment in some entity, other than as the holding of "constitutional" equity (shares etc.) in that entity.</skos:definition>
   </owl:Class>

   <owl:Class rdf:about="&fibo-be-oac-cpty;InvestmentBasedDeFactoControllingInterestParty">
      <rdfs:label>investment based de facto controlling interest party</rdfs:label>
      <skos:definition>A party which exercises some degree of de facto control based on some investment which they hold in the entity.</skos:definition>
      <rdfs:subClassOf rdf:resource="&fibo-be-oac-opty;Investor"/>
   </owl:Class>

   <owl:Class rdf:about="&fibo-be-oac-cpty;JointControllingParty">
      <rdfs:label>joint controlling party</rdfs:label>
      <rdfs:subClassOf rdf:resource="&fibo-be-oac-cpty;EntityControllingParty"/>
   </owl:Class>

   <owl:Class rdf:about="&fibo-be-oac-cpty;LimitedControllingParty">
      <rdfs:label>limited controlling party</rdfs:label>
      <skos:definition>Some individual entity which is able to direct the affairs of some business organization to a specific degree.</skos:definition>
   </owl:Class>

   <owl:Class rdf:about="&fibo-be-oac-cpty;LimitedDeFactoControl">
      <rdfs:label>limited de facto control</rdfs:label>
      <skos:definition>The ability to direct the affairs of some entity within prescribed limits. Those limits are described in terms of activities which the entity holding such control may cause the controlled entity to carry out.</skos:definition>
   </owl:Class>

   <owl:Class rdf:about="&fibo-be-oac-cpty;MajorityControllingParty">
      <rdfs:label>majority controlling party</rdfs:label>
      <rdfs:subClassOf rdf:resource="&fibo-be-oac-cpty;SoleControllingParty"/>
   </owl:Class>

   <owl:Class rdf:about="&fibo-be-oac-cpty;PartyHoldingSomeOptionForControl">
      <rdfs:label>party holding some option for control</rdfs:label>
      <skos:definition>Some party holding the option to exercise some De Jure Controlling Interest</skos:definition>
   </owl:Class>

   <owl:Class rdf:about="&fibo-be-oac-cpty;Receiver">
      <rdfs:label>receiver</rdfs:label>
      <skos:definition>A party appointed by some court for the purposes of winding up the affais of some entity which is no longer solvent.</skos:definition>
   </owl:Class>

   <owl:Class rdf:about="&fibo-be-oac-cpty;SignificantControllingInterestParty">
      <rdfs:label>significant controlling interest party</rdfs:label>
      <skos:definition>A person which owns a significant voting stake in this entity of between some lower significant threshold and 50%, but not 50% or more.</skos:definition>
   </owl:Class>

   <owl:Class rdf:about="&fibo-be-oac-cpty;SoleControllingParty">
      <rdfs:label>sole controlling party</rdfs:label>
      <skos:definition>Some individual entity which is able to direct the affairs of some business organization to some degree.</skos:definition>
   </owl:Class>

   <owl:Class rdf:about="&fibo-be-oac-cpty;TotalOwner">
      <rdfs:label>total owner</rdfs:label>
      <skos:definition>Entity having 100% ownership in the entity so owned.</skos:definition>
      <rdfs:subClassOf rdf:resource="&fibo-be-oac-opty;ConstitutionalOwner"/>
   </owl:Class>

   <owl:Class rdf:about="&fibo-be-oac-cpty;WarrantHolder">
      <rdfs:label>warrant holder</rdfs:label>
      <skos:definition>A holder of some warrant which when exercised would confer upon that party some de jure controlling interest in some entity.</skos:definition>
   </owl:Class>


  <!--
    ///////////////////////////////////////////////////////////////////////////////////////
    //
    // Individuals
    //
    ///////////////////////////////////////////////////////////////////////////////////////
    -->


<owl:NamedIndividual rdf:about="&fibo-be-oac-cpty;http...www.ecfr.gov.cgi-bin.retrieveECFR?gp=1&SID=156b3a57ae63855b0de1b32e322c998a&ty=HTML&h=L&r=PART&n=17y2.0.1.1.8#17.2.0.1.1.8.0.17.2">
      <rdfs:label>http://www.ecfr.gov/cgi-bin/retrieve e c f r?gp=1& s i d=156b3a57ae63855b0de1b32e322c998a&ty= h t m l&h= l&r= p a r t&n=17y2.0.1.1.8#17:2.0.1.1.8.0.17.2</rdfs:label>
      <rdf:type rdf:resource="&fibo-fnd-pub-pub;WebPage"/>
   </owl:NamedIndividual>

</rdf:RDF>