<?xml version="1.0" encoding="UTF-8"?>
  
<!DOCTYPE rdf:RDF [
    <!ENTITY fibo-be-oac-cown "http://spec.edmcouncil.org/fibo/red/be/ownership-and-control/corporate-ownership/">
    <!ENTITY fibo-fnd-agr-ctr "http://spec.edmcouncil.org/fibo/red/fnd/agreements/contracts/">
    <!ENTITY fibo-fnd-oac-own "http://spec.edmcouncil.org/fibo/red/fnd/ownership-and-control/ownership/">
    <!ENTITY fibo-be-corp-corp "http://spec.edmcouncil.org/fibo/red/be/corporations/corporations/">
    <!ENTITY fibo-sec-sec-ast "http://spec.edmcouncil.org/fibo/red/sec/securities/security-assets/">
    <!ENTITY fibo-fnd-acc-aeq "http://spec.edmcouncil.org/fibo/red/fnd/accounting/accounting-equity/">
    <!ENTITY fibo-be-oac-opty "http://spec.edmcouncil.org/fibo/red/be/ownership-and-control/ownership-parties/">
]>

<rdf:RDF xmlns:xsd="http://www.w3.org/2001/XMLSchema#"
         xmlns:sm="http://www.omg.org/techprocess/ab/SpecificationMetadata/"
         xmlns:xs="http://www.w3.org/2001/XMLSchema"
         xmlns:fibo-fnd-utl-av="http://www.omg.org/spec/EDMC-FIBO/FND/Utilities/AnnotationVocabulary/"
         xmlns:rdf="http://www.w3.org/1999/02/22-rdf-syntax-ns#"
         xmlns:rdfs="http://www.w3.org/2000/01/rdf-schema#"
         xmlns:owl="http://www.w3.org/2002/07/owl#"
         xmlns:skos="http://www.w3.org/2004/02/skos/core#"
         xmlns:dc="http://purl.org/dc/terms/"
         xml:base="http://spec.edmcouncil.org/fibo/red/be/ownership-and-control/corporate-ownership/">

   <owl:Ontology rdf:about="http://spec.edmcouncil.org/fibo/red/be/ownership-and-control/corporate-ownership/">
      <owl:imports rdf:resource="http://spec.edmcouncil.org/fibo/red/fnd/agreements/contracts/"/>
      <owl:imports rdf:resource="http://spec.edmcouncil.org/fibo/red/fnd/ownership-and-control/ownership/"/>
      <owl:imports rdf:resource="http://spec.edmcouncil.org/fibo/red/be/corporations/corporations/"/>
      <owl:imports rdf:resource="http://spec.edmcouncil.org/fibo/red/sec/securities/security-assets/"/>
      <owl:imports rdf:resource="http://spec.edmcouncil.org/fibo/red/fnd/accounting/accounting-equity/"/>
      <owl:imports rdf:resource="http://spec.edmcouncil.org/fibo/red/be/ownership-and-control/ownership-parties/"/>
   </owl:Ontology>


  <!--
    ///////////////////////////////////////////////////////////////////////////////////////
    //
    // Datatypes
    //
    ///////////////////////////////////////////////////////////////////////////////////////
    -->



  <!--
    ///////////////////////////////////////////////////////////////////////////////////////
    //
    // Object Properties
    //
    ///////////////////////////////////////////////////////////////////////////////////////
    -->


<owl:ObjectProperty rdf:about="&fibo-be-oac-cown;shareholderHoldsAnInterestIn">
      <rdfs:label>shareholder holds an interest in</rdfs:label>
      <skos:definition>The Shareholder owns some stake in the Incorporated company for example by virtue of owning some shares.</skos:definition>
      <rdfs:subPropertyOf rdf:resource="&fibo-be-oac-opty;holdsAnInterestIn"/>
      <rdfs:domain rdf:resource="&fibo-be-oac-cown;Shareholder"/>
      <rdfs:range rdf:resource="&fibo-be-corp-corp;IncorporatedCompany"/>
   </owl:ObjectProperty>

   <owl:ObjectProperty rdf:about="&fibo-be-oac-cown;shareholderHoldsEquity">
      <rdfs:label>shareholder holds equity</rdfs:label>
      <skos:definition>The shareholder holds some of the issued shareholder equity in the company, by way of the shares that they hold. This is a kind of Stockholders Equity.</skos:definition>
      <rdfs:subPropertyOf rdf:resource="&fibo-be-oac-opty;holdsSomeStockholderEquity"/>
      <rdfs:domain rdf:resource="&fibo-be-oac-cown;Shareholder"/>
      <rdfs:range rdf:resource="&fibo-fnd-acc-aeq;StockholdersEquity"/>
   </owl:ObjectProperty>

   <owl:ObjectProperty rdf:about="&fibo-be-oac-cown;heldBy">
      <rdfs:label>held by</rdfs:label>
      <skos:definition>The holder of the shares, that is the party of which this is the shareholding.</skos:definition>
      <rdfs:subPropertyOf rdf:resource="&fibo-fnd-oac-own;isAssetOf"/>
      <rdfs:subPropertyOf rdf:resource="&fibo-sec-sec-ast;heldBy"/>
      <rdfs:domain rdf:resource="&fibo-be-oac-cown;Shareholding"/>
      <rdfs:range rdf:resource="&fibo-be-oac-cown;Shareholder"/>
   </owl:ObjectProperty>


  <!--
    ///////////////////////////////////////////////////////////////////////////////////////
    //
    // Data Properties
    //
    ///////////////////////////////////////////////////////////////////////////////////////
    -->



  <!--
    ///////////////////////////////////////////////////////////////////////////////////////
    //
    // Annotation Properties
    //
    ///////////////////////////////////////////////////////////////////////////////////////
    -->



  <!--
    ///////////////////////////////////////////////////////////////////////////////////////
    //
    // Classes
    //
    ///////////////////////////////////////////////////////////////////////////////////////
    -->


<owl:Class rdf:about="&fibo-be-oac-cown;BeneficialOwner">
      <rdfs:label>beneficial owner</rdfs:label>
      <skos:definition>Some entity which owns some stake in the company (voting or non voting) and exercises some control either through that ownership or by some other means.</skos:definition>
      <rdfs:subClassOf rdf:resource="&fibo-be-oac-cown;Shareholder"/>
   </owl:Class>

   <owl:Class rdf:about="&fibo-be-oac-cown;PublicShareholder">
      <rdfs:label>public shareholder</rdfs:label>
      <skos:definition>A party that holds publicly issued shares in a listed company.</skos:definition>
   </owl:Class>

   <owl:Class rdf:about="&fibo-be-oac-cown;RegisteredShareholder">
      <rdfs:label>registered shareholder</rdfs:label>
      <skos:definition>A shareholder which is registered as such on the company shareholder register for that company.</skos:definition>
   </owl:Class>

   <owl:Class rdf:about="&fibo-be-oac-cown;Shareholder">
      <rdfs:label>shareholder</rdfs:label>
      <skos:definition>A party owning shares in some company limited by the issue of shares.</skos:definition>
      <rdfs:subClassOf rdf:resource="&fibo-fnd-agr-ctr;TransferableContractHolder"/>
      <rdfs:subClassOf rdf:resource="&fibo-sec-sec-ast;SecurityHolder"/>
      <rdfs:subClassOf rdf:resource="&fibo-be-oac-opty;ConstitutionalOwner"/>
   </owl:Class>

   <owl:Class rdf:about="&fibo-be-oac-cown;Shareholding">
      <rdfs:label>shareholding</rdfs:label>
      <skos:definition>The holding of some Share.</skos:definition>
      <rdfs:subClassOf rdf:resource="&fibo-sec-sec-ast;SecurityHolding"/>
      <rdfs:subClassOf rdf:resource="&fibo-fnd-oac-own;Asset"/>
   </owl:Class>


  <!--
    ///////////////////////////////////////////////////////////////////////////////////////
    //
    // Individuals
    //
    ///////////////////////////////////////////////////////////////////////////////////////
    -->


</rdf:RDF>