<?xml version="1.0" encoding="UTF-8"?>
  
<!DOCTYPE rdf:RDF [
    <!ENTITY fibo-be-oac-exec "http://spec.edmcouncil.org/fibo/red/be/ownership-and-control/executives/">
    <!ENTITY fibo-fnd-pty-pty "http://spec.edmcouncil.org/fibo/red/fnd/parties/parties/">
    <!ENTITY fibo-fnd-law-cor "http://spec.edmcouncil.org/fibo/red/fnd/law/legal-core/">
    <!ENTITY fibo-fnd-law-jur "http://spec.edmcouncil.org/fibo/red/fnd/law/jurisdictions/">
    <!ENTITY fibo-fnd-law-lcap "http://spec.edmcouncil.org/fibo/red/fnd/law/legal-capacities/">
    <!ENTITY fibo-fnd-oac-ctl "http://spec.edmcouncil.org/fibo/red/fnd/ownership-and-control/control/">
    <!ENTITY fibo-be-le-cb "http://spec.edmcouncil.org/fibo/red/be/legal-entities/corporate-bodies/">
    <!ENTITY fibo-rl-coll "http://spec.edmcouncil.org/fibo/red/fnd/relative/collections/">
    <!ENTITY fibo-be-corp-corp "http://spec.edmcouncil.org/fibo/red/be/corporations/corporations/">
    <!ENTITY fibo-fnd-org-fm "http://spec.edmcouncil.org/fibo/red/fnd/organizations/formal-organizations/">
    <!ENTITY fibo-be-le-lp "http://spec.edmcouncil.org/fibo/red/be/legal-entities/legal-persons/">
    <!ENTITY fibo-fnd-rel-rel "http://spec.edmcouncil.org/fibo/red/fnd/relations/relations/">
    <!ENTITY fibo-be-oac-cctl "http://spec.edmcouncil.org/fibo/red/be/ownership-and-control/corporate-control/">
    <!ENTITY fibo-be-oac-cpty "http://spec.edmcouncil.org/fibo/red/be/ownership-and-control/control-parties/">
]>

<rdf:RDF xmlns:xsd="http://www.w3.org/2001/XMLSchema#"
         xmlns:sm="http://www.omg.org/techprocess/ab/SpecificationMetadata/"
         xmlns:xs="http://www.w3.org/2001/XMLSchema"
         xmlns:fibo-fnd-utl-av="http://www.omg.org/spec/EDMC-FIBO/FND/Utilities/AnnotationVocabulary/"
         xmlns:rdf="http://www.w3.org/1999/02/22-rdf-syntax-ns#"
         xmlns:rdfs="http://www.w3.org/2000/01/rdf-schema#"
         xmlns:owl="http://www.w3.org/2002/07/owl#"
         xmlns:skos="http://www.w3.org/2004/02/skos/core#"
         xmlns:dc="http://purl.org/dc/terms/"
         xml:base="http://spec.edmcouncil.org/fibo/red/be/ownership-and-control/executives/">

   <owl:Ontology rdf:about="http://spec.edmcouncil.org/fibo/red/be/ownership-and-control/executives/">
      <owl:imports rdf:resource="http://spec.edmcouncil.org/fibo/red/fnd/parties/parties/"/>
      <owl:imports rdf:resource="http://spec.edmcouncil.org/fibo/red/fnd/law/legal-core/"/>
      <owl:imports rdf:resource="http://spec.edmcouncil.org/fibo/red/fnd/law/jurisdictions/"/>
      <owl:imports rdf:resource="http://spec.edmcouncil.org/fibo/red/fnd/law/legal-capacities/"/>
      <owl:imports rdf:resource="http://spec.edmcouncil.org/fibo/red/fnd/ownership-and-control/control/"/>
      <owl:imports rdf:resource="http://spec.edmcouncil.org/fibo/red/be/legal-entities/corporate-bodies/"/>
      <owl:imports rdf:resource="http://spec.edmcouncil.org/fibo/red/fnd/relative/collections/"/>
      <owl:imports rdf:resource="http://spec.edmcouncil.org/fibo/red/be/corporations/corporations/"/>
      <owl:imports rdf:resource="http://spec.edmcouncil.org/fibo/red/fnd/organizations/formal-organizations/"/>
      <owl:imports rdf:resource="http://spec.edmcouncil.org/fibo/red/be/legal-entities/legal-persons/"/>
      <owl:imports rdf:resource="http://spec.edmcouncil.org/fibo/red/fnd/relations/relations/"/>
      <owl:imports rdf:resource="http://spec.edmcouncil.org/fibo/red/be/ownership-and-control/corporate-control/"/>
      <owl:imports rdf:resource="http://spec.edmcouncil.org/fibo/red/be/ownership-and-control/control-parties/"/>
   </owl:Ontology>


  <!--
    ///////////////////////////////////////////////////////////////////////////////////////
    //
    // Datatypes
    //
    ///////////////////////////////////////////////////////////////////////////////////////
    -->



  <!--
    ///////////////////////////////////////////////////////////////////////////////////////
    //
    // Object Properties
    //
    ///////////////////////////////////////////////////////////////////////////////////////
    -->


<owl:ObjectProperty rdf:about="&fibo-be-oac-exec;boardCapacityIsConferredBy">
      <rdfs:label>board capacity is conferred by</rdfs:label>
      <skos:definition>The instrument which confers the Board Capacity. This is either the Company By-laws or the Board Agreement.</skos:definition>
      <rdfs:subPropertyOf rdf:resource="&fibo-fnd-law-lcap;isConferredBy"/>
      <rdfs:domain rdf:resource="&fibo-be-oac-exec;BoardCapacity"/>
      <rdfs:range rdf:resource="&fibo-be-oac-exec;.UnionClass.5"/>
   </owl:ObjectProperty>

   <owl:ObjectProperty rdf:about="&fibo-be-oac-exec;boardMemberIsAPartyTo">
      <rdfs:label>board member is a party to</rdfs:label>
      <rdfs:subPropertyOf rdf:resource="&fibo-fnd-pty-pty;isAPartyTo"/>
      <rdfs:domain rdf:resource="&fibo-be-oac-exec;BoardMember"/>
      <rdfs:range rdf:resource="&fibo-be-corp-corp;BoardAgreement"/>
   </owl:ObjectProperty>

   <owl:ObjectProperty rdf:about="&fibo-be-oac-exec;boardOfDirectorsAppoints">
      <rdfs:label>board of directors appoints</rdfs:label>
      <skos:definition>The board of the company has the power to appoint the individuals who are to be the public officers of the company.</skos:definition>
      <rdfs:subPropertyOf rdf:resource="&fibo-fnd-rel-rel;appoints"/>
      <rdfs:domain rdf:resource="&fibo-be-oac-exec;BoardOfDirectors"/>
      <rdfs:range rdf:resource="&fibo-be-oac-exec;CorporateOfficer"/>
   </owl:ObjectProperty>

   <owl:ObjectProperty rdf:about="&fibo-be-oac-exec;companyBoardHasVestedInIt">
      <rdfs:label>company board has vested in it</rdfs:label>
      <skos:definition>The board of a company has some legal capacity vested in it.</skos:definition>
      <rdfs:subPropertyOf rdf:resource="&fibo-fnd-law-lcap;hasCapacity"/>
      <rdfs:domain rdf:resource="&fibo-be-oac-exec;BoardOfDirectors"/>
      <rdfs:range rdf:resource="&fibo-be-oac-exec;BoardCapacity"/>
   </owl:ObjectProperty>

   <owl:ObjectProperty rdf:about="&fibo-be-oac-exec;boardOfDirectorsHasIdentity">
      <rdfs:label>board of directors has identity</rdfs:label>
      <rdfs:subPropertyOf rdf:resource="&fibo-fnd-pty-pty;hasIdentity"/>
      <rdfs:domain rdf:resource="&fibo-be-oac-exec;BoardOfDirectors"/>
      <rdfs:range rdf:resource="&fibo-fnd-org-fm;Group"/>
   </owl:ObjectProperty>

   <owl:ObjectProperty rdf:about="&fibo-be-oac-exec;boardOfDirectorsHasMember">
      <rdfs:label>board of directors has member</rdfs:label>
      <skos:definition>The board has a number of members who collectively exercise the powers of that board.</skos:definition>
      <rdfs:subPropertyOf rdf:resource="&fibo-rl-coll;hasConstituent"/>
      <rdfs:subPropertyOf rdf:resource="&fibo-fnd-rel-rel;hasMember"/>
      <rdfs:domain rdf:resource="&fibo-be-oac-exec;BoardOfDirectors"/>
      <rdfs:range rdf:resource="&fibo-be-oac-exec;BoardMember"/>
   </owl:ObjectProperty>

   <owl:ObjectProperty rdf:about="&fibo-be-oac-exec;constrains">
      <rdfs:label>constrains</rdfs:label>
      <skos:definition>The Instrument of Incorporation (being effectively the constitution of the entity) governs and constrains the application of the bylaws of the company.</skos:definition>
      <rdfs:subPropertyOf rdf:resource="&fibo-fnd-rel-rel;constrains"/>
      <rdfs:domain rdf:resource="&fibo-be-le-cb;InstrumentOfIncorporation"/>
      <rdfs:range rdf:resource="&fibo-be-oac-exec;CompanyBylaw"/>
   </owl:ObjectProperty>

   <owl:ObjectProperty rdf:about="&fibo-be-oac-exec;companyOfficerLegalCapacityConferredBy">
      <rdfs:label>company officer legal capacity conferred by</rdfs:label>
      <skos:definition>The capacity of the public officer is conferred by one or another ot the company legal form documentation (articles of association or equivalent) or some company by-law.</skos:definition>
      <rdfs:subPropertyOf rdf:resource="&fibo-fnd-law-lcap;isConferredBy"/>
      <rdfs:domain rdf:resource="&fibo-be-oac-exec;CorporateOfficerCapacity"/>
      <rdfs:range rdf:resource="&fibo-be-oac-exec;CompanyLaw"/>
   </owl:ObjectProperty>

   <owl:ObjectProperty rdf:about="&fibo-be-oac-exec;mandatedBy">
      <rdfs:label>mandated by</rdfs:label>
      <skos:definition>The Statutory Obligation is mandated by some piece of Company Law.</skos:definition>
      <rdfs:subPropertyOf rdf:resource="&fibo-fnd-law-lcap;statutoryResponsibilityIsMandatedBy"/>
      <rdfs:domain rdf:resource="&fibo-be-oac-exec;CompanyStatutoryObligation"/>
      <rdfs:range rdf:resource="&fibo-be-oac-exec;CompanyLaw"/>
   </owl:ObjectProperty>

   <owl:ObjectProperty rdf:about="&fibo-be-oac-exec;definedBy">
      <rdfs:label>defined by</rdfs:label>
      <skos:definition>The legal capacity of the Public Officer is set out in some piee of Company Law.</skos:definition>
      <rdfs:subPropertyOf rdf:resource="&fibo-fnd-rel-rel;isGoverneBy"/>
      <rdfs:domain rdf:resource="&fibo-be-oac-exec;CorporateOfficerCapacity"/>
      <rdfs:range rdf:resource="&fibo-be-oac-exec;CompanyLaw"/>
   </owl:ObjectProperty>

   <owl:ObjectProperty rdf:about="&fibo-be-oac-exec;publicOfficerIdentity">
      <rdfs:label>public officer identity</rdfs:label>
      <skos:definition>That which is the Public Officer. This must be a natural person and also must be an adult.</skos:definition>
      <rdfs:subPropertyOf rdf:resource="&fibo-be-oac-exec;legallyDelegatedAuthorityHasIdentity"/>
      <rdfs:domain rdf:resource="&fibo-be-oac-exec;CorporateOfficer"/>
      <rdfs:range rdf:resource="&fibo-be-le-lp;NaturalPerson"/>
   </owl:ObjectProperty>

   <owl:ObjectProperty rdf:about="&fibo-be-oac-exec;corporateOfficerHasResponsibility">
      <rdfs:label>corporate officer has responsibility</rdfs:label>
      <skos:definition>The Company Public Officer is party to some statutory obligations as mandated by the applicable body of Company Law.</skos:definition>
      <rdfs:subPropertyOf rdf:resource="&fibo-be-oac-exec;responsiblePartyHasResponsibility"/>
      <rdfs:domain rdf:resource="&fibo-be-oac-exec;CorporateOfficer"/>
      <rdfs:range rdf:resource="&fibo-be-oac-exec;CompanyStatutoryObligation"/>
   </owl:ObjectProperty>

   <owl:ObjectProperty rdf:about="&fibo-be-oac-exec;corporateOfficerHasResponsibilityDuty">
      <rdfs:label>corporate officer has responsibility duty</rdfs:label>
      <skos:definition>The Company Public Officer is party to some formally defined Public Officer Duty as set out on the relevant piece of Company Law.</skos:definition>
      <rdfs:subPropertyOf rdf:resource="&fibo-be-oac-exec;responsiblePartyHasResponsibility"/>
      <rdfs:domain rdf:resource="&fibo-be-oac-exec;CorporateOfficer"/>
      <rdfs:range rdf:resource="&fibo-be-oac-exec;CorporateOfficerDuty"/>
   </owl:ObjectProperty>

   <owl:ObjectProperty rdf:about="&fibo-be-oac-exec;deFactoControllingInterestPartyAppoints">
      <rdfs:label>de facto controlling interest party appoints</rdfs:label>
      <skos:definition>The Control Owner has some mechanism whereby they are able to vote and approve the board, other than through the mechanisms defined elsewhere.</skos:definition>
      <rdfs:subPropertyOf rdf:resource="&fibo-fnd-rel-rel;appoints"/>
      <rdfs:domain rdf:resource="&fibo-be-oac-cpty;DeFactoControllingInterestParty"/>
      <rdfs:range rdf:resource="&fibo-be-oac-exec;BoardMember"/>
   </owl:ObjectProperty>

   <owl:ObjectProperty rdf:about="&fibo-be-oac-exec;directorHasIdentity">
      <rdfs:label>director has identity</rdfs:label>
      <skos:definition>A board member (director) is typically a Natural Person, but may be any Legal Person.</skos:definition>
      <rdfs:subPropertyOf rdf:resource="&fibo-be-oac-exec;legallyDelegatedAuthorityHasIdentity"/>
      <rdfs:subPropertyOf rdf:resource="&fibo-fnd-pty-pty;hasIdentity"/>
      <rdfs:domain rdf:resource="&fibo-be-oac-exec;BoardMember"/>
      <rdfs:range rdf:resource="&fibo-be-le-lp;LegalPerson"/>
   </owl:ObjectProperty>

   <owl:ObjectProperty rdf:about="&fibo-be-oac-exec;executiveIdentity">
      <rdfs:label>executive identity</rdfs:label>
      <skos:definition>The Executive is some adult human being.</skos:definition>
      <rdfs:subPropertyOf rdf:resource="&fibo-be-oac-exec;legallyDelegatedAuthorityHasIdentity"/>
      <rdfs:domain rdf:resource="&fibo-be-oac-exec;Executive"/>
      <rdfs:range rdf:resource="&fibo-be-le-lp;NaturalPerson"/>
   </owl:ObjectProperty>

   <owl:ObjectProperty rdf:about="&fibo-be-oac-exec;legallyDelegatedAuthorityHasIdentity">
      <rdfs:label>legally delegated authority has identity</rdfs:label>
      <skos:definition>That which is in the role of Legally Controlling Party. This must be a Legal Person.</skos:definition>
      <rdfs:subPropertyOf rdf:resource="&fibo-fnd-pty-pty;hasIdentity"/>
      <rdfs:domain rdf:resource="&fibo-be-oac-exec;LegallyDelegatedAuthority"/>
      <rdfs:range rdf:resource="&fibo-be-le-lp;LegalPerson"/>
   </owl:ObjectProperty>

   <owl:ObjectProperty rdf:about="&fibo-be-oac-exec;responsiblePartyIdentity">
      <rdfs:label>responsible party identity</rdfs:label>
      <skos:definition>The Responsible Party must be some Natural Person.</skos:definition>
      <rdfs:subPropertyOf rdf:resource="&fibo-fnd-pty-pty;hasIdentity"/>
      <rdfs:domain rdf:resource="&fibo-be-oac-exec;ResponsibleParty"/>
      <rdfs:range rdf:resource="&fibo-be-le-lp;NaturalPerson"/>
   </owl:ObjectProperty>

   <owl:ObjectProperty rdf:about="&fibo-be-oac-exec;responsiblePartyHasResponsibility">
      <rdfs:label>responsible party has responsibility</rdfs:label>
      <skos:definition>The Responsible Party is deemed to be such because it is party to some formally defined Duty.</skos:definition>
      <rdfs:subPropertyOf rdf:resource="&fibo-be-oac-exec;hasReponsibility"/>
      <rdfs:domain rdf:resource="&fibo-be-oac-exec;ResponsibleParty"/>
      <rdfs:range rdf:resource="&fibo-fnd-law-lcap;Duty"/>
   </owl:ObjectProperty>

   <owl:ObjectProperty rdf:about="&fibo-be-oac-exec;votingShareholderElects">
      <rdfs:label>voting shareholder elects</rdfs:label>
      <skos:definition>The shareholders approve and vote for the members of the Board.</skos:definition>
      <rdfs:subPropertyOf rdf:resource="&fibo-be-oac-exec;elects"/>
      <rdfs:domain rdf:resource="&fibo-be-oac-cctl;VotingShareholder"/>
      <rdfs:range rdf:resource="&fibo-be-oac-exec;BoardMember"/>
   </owl:ObjectProperty>

   <owl:ObjectProperty rdf:about="&fibo-be-oac-exec;delegatesControlTo">
      <rdfs:label>delegates control to</rdfs:label>
      <skos:definition>The Organization which has management control of this Organization.</skos:definition>
      <rdfs:subPropertyOf rdf:resource="&fibo-fnd-rel-rel;designates"/>
      <rdfs:domain rdf:resource="&fibo-be-le-lp;LegalPerson"/>
      <rdfs:range rdf:resource="&fibo-be-oac-exec;LegallyDelegatedAuthority"/>
   </owl:ObjectProperty>

   <owl:ObjectProperty rdf:about="&fibo-be-oac-exec;elects">
      <rdfs:label>elects</rdfs:label>
      <rdfs:subPropertyOf rdf:resource="&fibo-fnd-rel-rel;designates"/>
      <rdfs:domain rdf:resource="&fibo-be-le-lp;LegalPerson"/>
      <rdfs:range rdf:resource="&fibo-be-le-lp;LegalPerson"/>
   </owl:ObjectProperty>

   <owl:ObjectProperty rdf:about="&fibo-be-oac-exec;hasCapacityCorporateOfficerCapacity">
      <rdfs:label>has capacity corporate officer capacity</rdfs:label>
      <skos:definition>The public officer of a company has some formal capacity vested in them.</skos:definition>
      <rdfs:subPropertyOf rdf:resource="&fibo-fnd-law-lcap;hasCapacity"/>
      <rdfs:domain rdf:resource="&fibo-be-oac-exec;CorporateOfficer"/>
      <rdfs:range rdf:resource="&fibo-be-oac-exec;CorporateOfficerCapacity"/>
   </owl:ObjectProperty>

   <owl:ObjectProperty rdf:about="&fibo-be-oac-exec;hasCapacitySignatoryCapacity">
      <rdfs:label>has capacity signatory capacity</rdfs:label>
      <skos:definition>The party which is a Company Public Officer is also defined as being a signatory in respect of the entity, that is the officer is able to sign agreements on the part of that entity.</skos:definition>
      <rdfs:subPropertyOf rdf:resource="&fibo-fnd-law-lcap;hasCapacity"/>
      <rdfs:domain rdf:resource="&fibo-be-oac-exec;CorporateOfficer"/>
      <rdfs:range rdf:resource="&fibo-fnd-law-lcap;SignatoryCapacity"/>
   </owl:ObjectProperty>

   <owl:ObjectProperty rdf:about="&fibo-be-oac-exec;hasDelegatedControlOf">
      <rdfs:label>has delegated control of</rdfs:label>
      <skos:definition>An organization of which this organization has control via some management structure.</skos:definition>
      <rdfs:domain rdf:resource="&fibo-be-oac-exec;LegallyDelegatedAuthority"/>
      <rdfs:range rdf:resource="&fibo-be-le-lp;LegalPerson"/>
   </owl:ObjectProperty>

   <owl:ObjectProperty rdf:about="&fibo-be-oac-exec;hasDelegatedControlOfItself">
      <rdfs:label>has delegated control of itself</rdfs:label>
      <rdfs:domain rdf:resource="&fibo-be-oac-exec;LegallyDelegatedAuthority"/>
      <rdfs:range rdf:resource="&fibo-be-le-lp;LegalPerson"/>
      <owl:inverseOf rdf:resource="&fibo-be-oac-exec;delegatesControlTo"/>
   </owl:ObjectProperty>

   <owl:ObjectProperty rdf:about="&fibo-be-oac-exec;hasReponsibility">
      <rdfs:label>has reponsibility</rdfs:label>
      <rdfs:domain rdf:resource="&fibo-fnd-rel-rel;Thing"/>
      <rdfs:range rdf:resource="&fibo-fnd-law-lcap;Duty"/>
   </owl:ObjectProperty>

   <owl:ObjectProperty rdf:about="&fibo-be-oac-exec;hasResponsibleParty">
      <rdfs:label>has responsible party</rdfs:label>
      <skos:definition>Some party having some defined responsibility in respect of the Formal Organization</skos:definition>
      <rdfs:subPropertyOf rdf:resource="&fibo-fnd-pty-pty;hasPartyInRole"/>
      <rdfs:domain rdf:resource="&fibo-fnd-org-fm;FormalOrganization"/>
      <rdfs:range rdf:resource="&fibo-be-oac-exec;ResponsibleParty"/>
   </owl:ObjectProperty>

   <owl:ObjectProperty rdf:about="&fibo-be-oac-exec;hasVestedInIt">
      <rdfs:label>has vested in it</rdfs:label>
      <skos:definition>A Delegated Legal Authority is one which has the legal capacity of Delegated Legal Authority vested in it.</skos:definition>
      <rdfs:subPropertyOf rdf:resource="&fibo-fnd-law-lcap;hasCapacity"/>
      <rdfs:domain rdf:resource="&fibo-be-oac-exec;LegallyDelegatedAuthority"/>
      <rdfs:range rdf:resource="&fibo-fnd-law-lcap;DelegatedLegalAuthority"/>
   </owl:ObjectProperty>

   <owl:ObjectProperty rdf:about="&fibo-be-oac-exec;mandatedByCompanyLaw">
      <rdfs:label>mandated by company law</rdfs:label>
      <skos:definition>The duties of a Company Public Officer are mandated by some applicable piece of Company Law.</skos:definition>
      <rdfs:subPropertyOf rdf:resource="&fibo-be-oac-exec;mandatedBy"/>
      <rdfs:domain rdf:resource="&fibo-be-oac-exec;CorporateOfficerDuty"/>
      <rdfs:range rdf:resource="&fibo-be-oac-exec;CompanyLaw"/>
   </owl:ObjectProperty>


  <!--
    ///////////////////////////////////////////////////////////////////////////////////////
    //
    // Data Properties
    //
    ///////////////////////////////////////////////////////////////////////////////////////
    -->



  <!--
    ///////////////////////////////////////////////////////////////////////////////////////
    //
    // Annotation Properties
    //
    ///////////////////////////////////////////////////////////////////////////////////////
    -->



  <!--
    ///////////////////////////////////////////////////////////////////////////////////////
    //
    // Classes
    //
    ///////////////////////////////////////////////////////////////////////////////////////
    -->


<owl:Class rdf:about="&fibo-be-oac-exec;.UnionClass.5">
      <skos:definition>The logical union of company legal form documents (Instrument of Incorporation, Memorandum and Articles or equivalent) and company by-laws.</skos:definition>
      <owl:equivalentClass>
         <owl:Class>
            <owl:unionOf rdf:parseType="Collection">
               <owl:Class rdf:about="&fibo-be-le-cb;InstrumentOfIncorporation"/>
               <owl:Class rdf:about="&fibo-be-oac-exec;CompanyBylaw"/>
               <owl:Class rdf:about="&fibo-be-corp-corp;BoardAgreement"/>
            </owl:unionOf>
         </owl:Class>
      </owl:equivalentClass>
   </owl:Class>

   <owl:Class rdf:about="&fibo-be-oac-exec;ArticlesOfIncorporation">
      <rdfs:label>articles of incorporation</rdfs:label>
      <skos:definition>The Articles of Association are a contract between the members and the organization, and among the members themselves, setting out the rights and duties of directors and stockholders individually and in meetings. Editorial Note: New definition and term (added in Executives) arrived at during OMG OWL migration process. Known then as "Incorporated Company Legal form Documentation" (seeking a jurisdiction neutral label). Original working definition: "The articles of association which are defined when a registered company (specifically a company limited by the issue of shares) is set up. " Explanatory Note: In some (or all?) Jurisdictions the articles in the company constitution become terms of the contract which is a share in that company. Example: In the UK: Memorandum and Articles of Association make up the Constitution. Bits of that are defined by law. In Delaware you have to have 3 officers which may be the same individual. Other states they must be separate individuals. Also in Delaware they need not be American citizens, in other states they must. Minimum requirements to be met. Also this may change as law changes. See also Anti ML and KYC stuff. Schools - governing bodies, their constitutions. Trusts.</skos:definition>
      <rdfs:subClassOf rdf:resource="&fibo-be-le-cb;InstrumentOfIncorporation"/>
   </owl:Class>

   <owl:Class rdf:about="&fibo-be-oac-exec;Auditor">
      <rdfs:label>auditor</rdfs:label>
      <skos:definition>The auditor of the company is a public officer which is responsible for reporting on the financial situation of the company.</skos:definition>
      <rdfs:subClassOf rdf:resource="&fibo-be-oac-exec;ResponsibleParty"/>
   </owl:Class>

   <owl:Class rdf:about="&fibo-be-oac-exec;BoardCapacity">
      <rdfs:label>board capacity</rdfs:label>
      <skos:definition>The capacity which resides in the Board of Directors of a company.</skos:definition>
      <rdfs:subClassOf rdf:resource="&fibo-fnd-law-lcap;DelegatedLegalAuthority"/>
   </owl:Class>

   <owl:Class rdf:about="&fibo-be-oac-exec;BoardMember">
      <rdfs:label>board member</rdfs:label>
      <skos:definition>A person who is a member of the Board of Directors of some Incorporated company.</skos:definition>
      <rdfs:subClassOf rdf:resource="&fibo-fnd-pty-pty;OrganizationMember"/>
      <rdfs:subClassOf rdf:resource="&fibo-be-oac-exec;LegallyDelegatedAuthority"/>
   </owl:Class>

   <owl:Class rdf:about="&fibo-be-oac-exec;BoardOfDirectors">
      <rdfs:label>board of directors</rdfs:label>
      <skos:definition>The group of entities defined as being the Board of Directors of the company.</skos:definition>
      <rdfs:subClassOf rdf:resource="&fibo-be-oac-cpty;EntityControllingParty"/>
   </owl:Class>

   <owl:Class rdf:about="&fibo-be-oac-exec;Bylaw">
      <rdfs:label>bylaw</rdfs:label>
      <skos:definition>The bylaws of some commercial or other registered enterprise.</skos:definition>
      <rdfs:subClassOf rdf:resource="&fibo-fnd-law-cor;Law"/>
   </owl:Class>

   <owl:Class rdf:about="&fibo-be-oac-exec;ChiefExecutiveOfficer">
      <rdfs:label>chief executive officer</rdfs:label>
      <skos:definition>Some person performing the role of Chief Executive Officer of a company, with the responsibilities and rights defined for that party in the relevant statutes.</skos:definition>
      <rdfs:subClassOf rdf:resource="&fibo-be-oac-exec;ExecutiveBoardMember"/>
      <rdfs:subClassOf rdf:resource="&fibo-be-oac-exec;CorporateOfficer"/>
   </owl:Class>

   <owl:Class rdf:about="&fibo-be-oac-exec;ChiefFinancialOfficer">
      <rdfs:label>chief financial officer</rdfs:label>
      <skos:definition>Some person performing the role of Chief Financial Officer of a company, with the responsibilities and rights defined for that party in the relevant statutes.</skos:definition>
      <rdfs:subClassOf rdf:resource="&fibo-be-oac-exec;Executive"/>
   </owl:Class>

   <owl:Class rdf:about="&fibo-be-oac-exec;CompanyBylaw">
      <rdfs:label>company bylaw</rdfs:label>
      <skos:definition>A by-law of a company.</skos:definition>
      <rdfs:subClassOf rdf:resource="&fibo-be-oac-exec;Bylaw"/>
   </owl:Class>

   <owl:Class rdf:about="&fibo-be-oac-exec;CompanyLaw">
      <rdfs:label>company law</rdfs:label>
      <skos:definition>The law dealing with companies in a given jurisdiction.</skos:definition>
      <rdfs:subClassOf rdf:resource="&fibo-fnd-law-jur;StatuteLaw"/>
   </owl:Class>

   <owl:Class rdf:about="&fibo-be-oac-exec;CompanySecretary">
      <rdfs:label>company secretary</rdfs:label>
      <skos:definition>Formal definition required</skos:definition>
   </owl:Class>

   <owl:Class rdf:about="&fibo-be-oac-exec;CompanyStatutoryObligation">
      <rdfs:label>company statutory obligation</rdfs:label>
      <skos:definition>An obligation defined in company law (statute).</skos:definition>
      <rdfs:subClassOf rdf:resource="&fibo-fnd-law-lcap;StatutoryResponsibility"/>
   </owl:Class>

   <owl:Class rdf:about="&fibo-be-oac-exec;CorporateOfficer">
      <rdfs:label>corporate officer</rdfs:label>
      <skos:definition>Some party which is recognized by law as having the role and responsibilities defined for a Public Officer as described in that law.</skos:definition>
   </owl:Class>

   <owl:Class rdf:about="&fibo-be-oac-exec;CorporateOfficerCapacity">
      <rdfs:label>corporate officer capacity</rdfs:label>
      <skos:definition>The capacity vested in a public officer of a company. Further notes: This is framed as a capacity: Individual acts in their capacity of the role as CFO, CEO etc. but their legal liability rests in their relationship with the board itself i.e. comes from their membership on the board from a corporate standpoint. Scope Note: Originally framed with reference to Incorporated company, this term and its related terms have been re-framed as applying to any Body Corporate. May be specialized for Incorporated Companies and other Bodies Corporate at some future point.</skos:definition>
   </owl:Class>

   <owl:Class rdf:about="&fibo-be-oac-exec;CorporateOfficerDuty">
      <rdfs:label>corporate officer duty</rdfs:label>
      <skos:definition>Some duty incumbent upon some public officer of a company.</skos:definition>
      <rdfs:subClassOf rdf:resource="&fibo-be-oac-exec;CompanyStatutoryObligation"/>
   </owl:Class>

   <owl:Class rdf:about="&fibo-be-oac-exec;Executive">
      <rdfs:label>executive</rdfs:label>
      <skos:definition>Some person in whom some level of management control of some organization has been conferred. Further Notes The owners of a business delegate their controlling parties ot controlling parties which gives them the right to control. These rights are reassigned by the creditors in the event of a business being under receivership.</skos:definition>
   </owl:Class>

   <owl:Class rdf:about="&fibo-be-oac-exec;ExecutiveBoardMember">
      <rdfs:label>executive board member</rdfs:label>
      <skos:definition>Some person performing the role of a Board Member of a company, and being one with some executive responsibilities within that company.</skos:definition>
      <rdfs:subClassOf rdf:resource="&fibo-be-oac-exec;BoardMember"/>
   </owl:Class>

   <owl:Class rdf:about="&fibo-be-oac-exec;LegallyDelegatedAuthority">
      <rdfs:label>legally delegated authority</rdfs:label>
      <skos:definition>A party having some legal control of some entity.</skos:definition>
      <rdfs:subClassOf rdf:resource="&fibo-fnd-oac-ctl;ControllingParty"/>
   </owl:Class>

   <owl:Class rdf:about="&fibo-be-oac-exec;NonExecutiveBoardMember">
      <rdfs:label>non executive board member</rdfs:label>
      <skos:definition>Some person performing the role of a Board Member of a company, and having no executive responsibilities towards the running of the company.</skos:definition>
   </owl:Class>

   <owl:Class rdf:about="&fibo-be-oac-exec;ResponsibleParty">
      <rdfs:label>responsible party</rdfs:label>
      <skos:definition>A Party to which some responsibility has been given.</skos:definition>
      <rdfs:subClassOf rdf:resource="&fibo-fnd-pty-pty;PartyInRole"/>
   </owl:Class>


  <!--
    ///////////////////////////////////////////////////////////////////////////////////////
    //
    // Individuals
    //
    ///////////////////////////////////////////////////////////////////////////////////////
    -->


</rdf:RDF>