<?xml version="1.0" encoding="UTF-8"?>
  
<!DOCTYPE rdf:RDF [
    <!ENTITY fibo-be-oac-opty "http://spec.edmcouncil.org/fibo/red/be/ownership-and-control/ownership-parties/">
    <!ENTITY fibo-fnd-agr-ctr "http://spec.edmcouncil.org/fibo/red/fnd/agreements/contracts/">
    <!ENTITY fibo-fnd-oac-own "http://spec.edmcouncil.org/fibo/red/fnd/ownership-and-control/ownership/">
    <!ENTITY fibo-fnd-acc-aeq "http://spec.edmcouncil.org/fibo/red/fnd/accounting/accounting-equity/">
    <!ENTITY fibo-be-le-fbo "http://spec.edmcouncil.org/fibo/red/be/legal-entities/formal-business-organizations/">
    <!ENTITY fibo-fnd-rl-prx "http://spec.edmcouncil.org/fibo/red/fnd/relative/party-extensions/">
    <!ENTITY fibo-fnd-pty-pty "http://spec.edmcouncil.org/fibo/red/fnd/parties/parties/">
    <!ENTITY fibo-fnd-oac-ctl "http://spec.edmcouncil.org/fibo/red/fnd/ownership-and-control/control/">
    <!ENTITY fibo-be-le-cb "http://spec.edmcouncil.org/fibo/red/be/legal-entities/corporate-bodies/">
    <!ENTITY fibo-fnd-rel-rel "http://spec.edmcouncil.org/fibo/red/fnd/relations/relations/">
]>

<rdf:RDF xmlns:xsd="http://www.w3.org/2001/XMLSchema#"
         xmlns:sm="http://www.omg.org/techprocess/ab/SpecificationMetadata/"
         xmlns:xs="http://www.w3.org/2001/XMLSchema"
         xmlns:fibo-fnd-utl-av="http://www.omg.org/spec/EDMC-FIBO/FND/Utilities/AnnotationVocabulary/"
         xmlns:rdf="http://www.w3.org/1999/02/22-rdf-syntax-ns#"
         xmlns:rdfs="http://www.w3.org/2000/01/rdf-schema#"
         xmlns:owl="http://www.w3.org/2002/07/owl#"
         xmlns:skos="http://www.w3.org/2004/02/skos/core#"
         xmlns:dc="http://purl.org/dc/terms/"
         xml:base="http://spec.edmcouncil.org/fibo/red/be/ownership-and-control/ownership-parties/">

   <owl:Ontology rdf:about="http://spec.edmcouncil.org/fibo/red/be/ownership-and-control/ownership-parties/">
      <owl:imports rdf:resource="http://spec.edmcouncil.org/fibo/red/fnd/agreements/contracts/"/>
      <owl:imports rdf:resource="http://spec.edmcouncil.org/fibo/red/fnd/ownership-and-control/ownership/"/>
      <owl:imports rdf:resource="http://spec.edmcouncil.org/fibo/red/fnd/accounting/accounting-equity/"/>
      <owl:imports rdf:resource="http://spec.edmcouncil.org/fibo/red/be/legal-entities/formal-business-organizations/"/>
      <owl:imports rdf:resource="http://spec.edmcouncil.org/fibo/red/fnd/relative/party-extensions/"/>
      <owl:imports rdf:resource="http://spec.edmcouncil.org/fibo/red/fnd/parties/parties/"/>
      <owl:imports rdf:resource="http://spec.edmcouncil.org/fibo/red/fnd/ownership-and-control/control/"/>
      <owl:imports rdf:resource="http://spec.edmcouncil.org/fibo/red/be/legal-entities/corporate-bodies/"/>
      <owl:imports rdf:resource="http://spec.edmcouncil.org/fibo/red/fnd/relations/relations/"/>
   </owl:Ontology>


  <!--
    ///////////////////////////////////////////////////////////////////////////////////////
    //
    // Datatypes
    //
    ///////////////////////////////////////////////////////////////////////////////////////
    -->



  <!--
    ///////////////////////////////////////////////////////////////////////////////////////
    //
    // Object Properties
    //
    ///////////////////////////////////////////////////////////////////////////////////////
    -->


<owl:ObjectProperty rdf:about="&fibo-be-oac-opty;constitutionalOwnerHoldsAnInterestIn">
      <rdfs:label>constitutional owner holds an interest in</rdfs:label>
      <rdfs:subPropertyOf rdf:resource="&fibo-be-oac-opty;holdsAnInterestIn"/>
      <rdfs:domain rdf:resource="&fibo-be-oac-opty;ConstitutionalOwner"/>
      <rdfs:range rdf:resource="&fibo-be-le-fbo;FormallyConstitutedOrganization"/>
   </owl:ObjectProperty>

   <owl:ObjectProperty rdf:about="&fibo-be-oac-opty;equityIsEquityHeldBy">
      <rdfs:label>equity is equity held by</rdfs:label>
      <rdfs:subPropertyOf rdf:resource="&fibo-be-oac-opty;isEquityHeldBy"/>
      <rdfs:domain rdf:resource="&fibo-fnd-acc-aeq;Equity"/>
      <rdfs:range rdf:resource="&fibo-be-oac-opty;EntityOwner"/>
      <owl:inverseOf rdf:resource="&fibo-be-oac-opty;holdsEquity"/>
   </owl:ObjectProperty>

   <owl:ObjectProperty rdf:about="&fibo-be-oac-opty;guaranteeProvidingMemberGuarantees">
      <rdfs:label>guarantee providing member guarantees</rdfs:label>
      <skos:definition>Guarantee Providing Member provides a formal assurance or promise, esp. that certain conditions shall be fulfilled relating to a product, service, or transaction, in respect of the Body Incorporated by Guarantee.</skos:definition>
      <rdfs:subPropertyOf rdf:resource="&fibo-be-oac-opty;guarantees"/>
      <rdfs:domain rdf:resource="&fibo-be-oac-opty;GuaranteeProvidingMember"/>
      <rdfs:range rdf:resource="&fibo-be-le-cb;BodyIncorporatedWithGuarantee"/>
   </owl:ObjectProperty>

   <owl:ObjectProperty rdf:about="&fibo-be-oac-opty;guarantorHasIdentity">
      <rdfs:label>guarantor has identity</rdfs:label>
      <skos:definition>The entity which performs the role of the Guarantor.</skos:definition>
      <rdfs:subPropertyOf rdf:resource="&fibo-fnd-pty-pty;hasIdentity"/>
      <rdfs:subPropertyOf rdf:resource="&fibo-fnd-rl-prx;organizationMemberHasIdentity"/>
      <rdfs:domain rdf:resource="&fibo-be-oac-opty;GuaranteeProvidingMember"/>
      <rdfs:range rdf:resource="&fibo-fnd-pty-pty;IndependentParty"/>
   </owl:ObjectProperty>

   <owl:ObjectProperty rdf:about="&fibo-be-oac-opty;investmentEquityIsEquityHelodBy">
      <rdfs:label>investment equity is equity helod by</rdfs:label>
      <skos:definition>Investment is invested by a party which, by virtue of holding some equity investment in the entity, has some ownership stake in it.</skos:definition>
      <rdfs:subPropertyOf rdf:resource="&fibo-be-oac-opty;isEquityHeldBy"/>
      <rdfs:domain rdf:resource="&fibo-be-oac-opty;InvestmentEquity"/>
      <rdfs:range rdf:resource="&fibo-be-oac-opty;Investor"/>
   </owl:ObjectProperty>

   <owl:ObjectProperty rdf:about="&fibo-be-oac-opty;setsOutTermsForInvestmentEquity">
      <rdfs:label>sets out terms for investment equity</rdfs:label>
      <skos:definition>The Contract sets out the terms for the Investment Equity in the entity, setting out the rights which are conferred on any investor in that equity.</skos:definition>
      <rdfs:subPropertyOf rdf:resource="&fibo-fnd-agr-ctr;definesTermsFor"/>
      <rdfs:domain rdf:resource="&fibo-be-oac-opty;InvestorContract"/>
      <rdfs:range rdf:resource="&fibo-be-oac-opty;InvestmentEquity"/>
   </owl:ObjectProperty>

   <owl:ObjectProperty rdf:about="&fibo-be-oac-opty;investorHoldsAnInterestIn">
      <rdfs:label>investor holds an interest in</rdfs:label>
      <rdfs:subPropertyOf rdf:resource="&fibo-be-oac-opty;holdsAnInterestIn"/>
      <rdfs:domain rdf:resource="&fibo-be-oac-opty;Investor"/>
      <rdfs:range rdf:resource="&fibo-be-le-fbo;FormallyConstitutedOrganization"/>
   </owl:ObjectProperty>

   <owl:ObjectProperty rdf:about="&fibo-be-oac-opty;confers">
      <rdfs:label>confers</rdfs:label>
      <skos:definition>The equity confers some controlling interest on the holder of that equity.</skos:definition>
      <rdfs:subPropertyOf rdf:resource="&fibo-fnd-rel-rel;confers"/>
      <rdfs:domain rdf:resource="&fibo-be-oac-opty;ControllingEquity"/>
      <rdfs:range rdf:resource="&fibo-fnd-oac-ctl;DeJureControl"/>
   </owl:ObjectProperty>

   <owl:ObjectProperty rdf:about="&fibo-be-oac-opty;guarantees">
      <rdfs:label>guarantees</rdfs:label>
      <skos:definition>provide a formal assurance or promise, esp. that certain conditions shall be fulfilled relating to a product, service, or transaction</skos:definition>
      <rdfs:domain rdf:resource="&fibo-fnd-rel-rel;Thing"/>
      <rdfs:range rdf:resource="&fibo-fnd-rel-rel;Thing"/>
   </owl:ObjectProperty>

   <owl:ObjectProperty rdf:about="&fibo-be-oac-opty;hasConstitutionalOwner">
      <rdfs:label>has constitutional owner</rdfs:label>
      <skos:definition>links a constitutional interest/position in something (e.g., a formal business organization) to the party that holds or owns it, in whole or in part</skos:definition>
      <rdfs:subPropertyOf rdf:resource="&fibo-be-oac-opty;entityOwnedBy"/>
      <rdfs:domain rdf:resource="&fibo-be-le-fbo;FormallyConstitutedOrganization"/>
      <rdfs:range rdf:resource="&fibo-be-oac-opty;ConstitutionalOwner"/>
   </owl:ObjectProperty>

   <owl:ObjectProperty rdf:about="&fibo-be-oac-opty;hasInvestor">
      <rdfs:label>has investor</rdfs:label>
      <skos:definition>links an investment interest in something (e.g., a formal business organization) to the party that holds or owns it, in whole or in part</skos:definition>
      <rdfs:subPropertyOf rdf:resource="&fibo-be-oac-opty;entityOwnedBy"/>
      <rdfs:domain rdf:resource="&fibo-be-le-fbo;FormallyConstitutedOrganization"/>
      <rdfs:range rdf:resource="&fibo-be-oac-opty;Investor"/>
   </owl:ObjectProperty>

   <owl:ObjectProperty rdf:about="&fibo-be-oac-opty;holdsSomeInvestmentEquity">
      <rdfs:label>holds some investment equity</rdfs:label>
      <skos:definition>Some equity held by the investor in the form of investment equity.</skos:definition>
      <rdfs:subPropertyOf rdf:resource="&fibo-be-oac-opty;holdsEquity"/>
      <rdfs:domain rdf:resource="&fibo-be-oac-opty;Investor"/>
      <rdfs:range rdf:resource="&fibo-be-oac-opty;InvestmentEquity"/>
   </owl:ObjectProperty>

   <owl:ObjectProperty rdf:about="&fibo-be-oac-opty;holdsSomeStockholderEquity">
      <rdfs:label>holds some stockholder equity</rdfs:label>
      <skos:definition>A Constitutional Owning Party is defined as such by the fact that they hold some portion of the Stockholder Equity in that entity.</skos:definition>
      <rdfs:subPropertyOf rdf:resource="&fibo-be-oac-opty;holdsEquity"/>
      <rdfs:domain rdf:resource="&fibo-be-oac-opty;ConstitutionalOwner"/>
      <rdfs:range rdf:resource="&fibo-fnd-acc-aeq;StockholdersEquity"/>
   </owl:ObjectProperty>

   <owl:ObjectProperty rdf:about="&fibo-be-oac-opty;holdsAnInterestIn">
      <rdfs:label>holds an interest in</rdfs:label>
      <skos:definition>links a party to some organization it holds an interest in</skos:definition>
      <rdfs:subPropertyOf rdf:resource="&fibo-fnd-oac-own;owns"/>
      <rdfs:domain rdf:resource="&fibo-be-oac-opty;EntityOwner"/>
      <rdfs:range rdf:resource="&fibo-be-le-fbo;FormallyConstitutedOrganization"/>
   </owl:ObjectProperty>

   <owl:ObjectProperty rdf:about="&fibo-be-oac-opty;holdsEquity">
      <rdfs:label>holds equity</rdfs:label>
      <skos:definition>links a party to some equity it holds</skos:definition>
      <rdfs:subPropertyOf rdf:resource="&fibo-fnd-oac-own;owns"/>
      <rdfs:domain rdf:resource="&fibo-be-oac-opty;EntityOwner"/>
      <rdfs:range rdf:resource="&fibo-fnd-acc-aeq;Equity"/>
   </owl:ObjectProperty>

   <owl:ObjectProperty rdf:about="&fibo-be-oac-opty;involvesEntityOwningParty">
      <rdfs:label>involves entity owning party</rdfs:label>
      <skos:definition>Entity ownership involves some party which is identified as an Entity Owning Party.</skos:definition>
      <rdfs:subPropertyOf rdf:resource="&fibo-fnd-oac-own;ownershipInvolves"/>
      <rdfs:domain rdf:resource="&fibo-be-oac-opty;EntityOwnershipContext"/>
      <rdfs:range rdf:resource="&fibo-be-oac-opty;EntityOwner"/>
   </owl:ObjectProperty>

   <owl:ObjectProperty rdf:about="&fibo-be-oac-opty;isEquityHeldBy">
      <rdfs:label>is equity held by</rdfs:label>
      <skos:definition>links some equity to the party that holds it</skos:definition>
      <rdfs:subPropertyOf rdf:resource="&fibo-fnd-oac-own;isOwnedBy"/>
      <rdfs:domain rdf:resource="http://www.w3.org/2002/07/owl#Thing"/>
      <rdfs:range rdf:resource="&fibo-be-oac-opty;EntityOwner"/>
   </owl:ObjectProperty>

   <owl:ObjectProperty rdf:about="&fibo-be-oac-opty;entityOwnedBy">
      <rdfs:label>entity owned by</rdfs:label>
      <rdfs:subPropertyOf rdf:resource="&fibo-fnd-oac-own;isOwnedBy"/>
      <rdfs:domain rdf:resource="&fibo-be-le-fbo;FormallyConstitutedOrganization"/>
      <rdfs:range rdf:resource="&fibo-be-oac-opty;EntityOwner"/>
      <owl:inverseOf rdf:resource="&fibo-be-oac-opty;holdsAnInterestIn"/>
   </owl:ObjectProperty>


  <!--
    ///////////////////////////////////////////////////////////////////////////////////////
    //
    // Data Properties
    //
    ///////////////////////////////////////////////////////////////////////////////////////
    -->



  <!--
    ///////////////////////////////////////////////////////////////////////////////////////
    //
    // Annotation Properties
    //
    ///////////////////////////////////////////////////////////////////////////////////////
    -->



  <!--
    ///////////////////////////////////////////////////////////////////////////////////////
    //
    // Classes
    //
    ///////////////////////////////////////////////////////////////////////////////////////
    -->


<owl:Class rdf:about="&fibo-be-oac-opty;ConstitutionalOwner">
      <rdfs:label>constitutional owner</rdfs:label>
      <skos:definition>A party which owns some equity stake in some entity, which is some part of the formal equity make-up of that entity, such as shares or general partner equity.</skos:definition>
      <rdfs:subClassOf rdf:resource="&fibo-be-oac-opty;EntityOwner"/>
   </owl:Class>

   <owl:Class rdf:about="&fibo-be-oac-opty;ControllingEquity">
      <rdfs:label>controlling equity</rdfs:label>
      <skos:definition>Equity which brings with it some form of de jure control of the entity in which it represents and interest.</skos:definition>
      <rdfs:subClassOf rdf:resource="&fibo-fnd-acc-aeq;StockholdersEquity"/>
   </owl:Class>

   <owl:Class rdf:about="&fibo-be-oac-opty;EntityOwner">
      <rdfs:label>entity owner</rdfs:label>
      <skos:definition>A party having some ownership in some entity.</skos:definition>
      <rdfs:subClassOf rdf:resource="&fibo-fnd-oac-own;Owner"/>
   </owl:Class>

   <owl:Class rdf:about="&fibo-be-oac-opty;EntityOwnershipContext">
      <rdfs:label>entity ownership context</rdfs:label>
      <skos:definition>The context of ownership by some party of an interest in some Formal Organization.</skos:definition>
      <rdfs:subClassOf rdf:resource="&fibo-fnd-oac-own;Ownership"/>
   </owl:Class>

   <owl:Class rdf:about="&fibo-be-oac-opty;GuaranteeProvidingMember">
      <rdfs:label>guarantee providing member</rdfs:label>
      <skos:definition>An entity which has issued some Guarantee for a body incorporated by the issuance of Guarantees.</skos:definition>
      <rdfs:subClassOf rdf:resource="&fibo-be-le-fbo;FormalBusinessOrganizationMember"/>
   </owl:Class>

   <owl:Class rdf:about="&fibo-be-oac-opty;InvestmentEquity">
      <rdfs:label>investment equity</rdfs:label>
      <skos:definition>Equity which represents some investment in some entity, but which may or may not take the form of stockholder equity.</skos:definition>
      <rdfs:subClassOf rdf:resource="&fibo-fnd-acc-aeq;Equity"/>
   </owl:Class>

   <owl:Class rdf:about="&fibo-be-oac-opty;Investor">
      <rdfs:label>investor</rdfs:label>
      <skos:definition>A party which owns some stake in some organization by way of investment.</skos:definition>
   </owl:Class>

   <owl:Class rdf:about="&fibo-be-oac-opty;InvestorContract">
      <rdfs:label>investor contract</rdfs:label>
      <skos:definition>Contract setting out the terms under which some investor invests in the entity and setting out the rights which are conferred on that investor.</skos:definition>
      <rdfs:subClassOf rdf:resource="&fibo-fnd-agr-ctr;WrittenContract"/>
   </owl:Class>


  <!--
    ///////////////////////////////////////////////////////////////////////////////////////
    //
    // Individuals
    //
    ///////////////////////////////////////////////////////////////////////////////////////
    -->


</rdf:RDF>