<?xml version="1.0" encoding="UTF-8"?>
<!DOCTYPE rdf:RDF [
	<!ENTITY dct "http://purl.org/dc/terms/">
	<!ENTITY fibo-be-ge-ge "https://spec.edmcouncil.org/fibo/ontology/BE/GovernmentEntities/GovernmentEntities/">
	<!ENTITY fibo-be-le-cb "https://spec.edmcouncil.org/fibo/ontology/BE/LegalEntities/CorporateBodies/">
	<!ENTITY fibo-be-le-lp "https://spec.edmcouncil.org/fibo/ontology/BE/LegalEntities/LegalPersons/">
	<!ENTITY fibo-fbc-dae-dbt "https://spec.edmcouncil.org/fibo/ontology/FBC/DebtAndEquities/Debt/">
	<!ENTITY fibo-fbc-dae-gty "https://spec.edmcouncil.org/fibo/ontology/FBC/DebtAndEquities/Guaranty/">
	<!ENTITY fibo-fbc-fi-fi "https://spec.edmcouncil.org/fibo/ontology/FBC/FinancialInstruments/FinancialInstruments/">
	<!ENTITY fibo-fbc-pas-fpas "https://spec.edmcouncil.org/fibo/ontology/FBC/ProductsAndServices/FinancialProductsAndServices/">
	<!ENTITY fibo-fnd-acc-cur "https://spec.edmcouncil.org/fibo/ontology/FND/Accounting/CurrencyAmount/">
	<!ENTITY fibo-fnd-agr-agr "https://spec.edmcouncil.org/fibo/ontology/FND/Agreements/Agreements/">
	<!ENTITY fibo-fnd-agr-ctr "https://spec.edmcouncil.org/fibo/ontology/FND/Agreements/Contracts/">
	<!ENTITY fibo-fnd-dt-bd "https://spec.edmcouncil.org/fibo/ontology/FND/DatesAndTimes/BusinessDates/">
	<!ENTITY fibo-fnd-dt-fd "https://spec.edmcouncil.org/fibo/ontology/FND/DatesAndTimes/FinancialDates/">
	<!ENTITY fibo-fnd-dt-oc "https://spec.edmcouncil.org/fibo/ontology/FND/DatesAndTimes/Occurrences/">
	<!ENTITY fibo-fnd-pas-psch "https://spec.edmcouncil.org/fibo/ontology/FND/ProductsAndServices/PaymentsAndSchedules/">
	<!ENTITY fibo-fnd-pty-rl "https://spec.edmcouncil.org/fibo/ontology/FND/Parties/Roles/">
	<!ENTITY fibo-fnd-rel-rel "https://spec.edmcouncil.org/fibo/ontology/FND/Relations/Relations/">
	<!ENTITY fibo-fnd-utl-alx "https://spec.edmcouncil.org/fibo/ontology/FND/Utilities/Analytics/">
	<!ENTITY fibo-fnd-utl-av "https://spec.edmcouncil.org/fibo/ontology/FND/Utilities/AnnotationVocabulary/">
	<!ENTITY fibo-fnd-utl-val "https://spec.edmcouncil.org/fibo/ontology/FND/Utilities/Values/">
	<!ENTITY fibo-ind-ei-ei "https://spec.edmcouncil.org/fibo/ontology/IND/EconomicIndicators/EconomicIndicators/">
	<!ENTITY fibo-ind-ind-ind "https://spec.edmcouncil.org/fibo/ontology/IND/Indicators/Indicators/">
	<!ENTITY fibo-ind-ir-ir "https://spec.edmcouncil.org/fibo/ontology/IND/InterestRates/InterestRates/">
	<!ENTITY fibo-sec-dbt-bnd "https://spec.edmcouncil.org/fibo/ontology/SEC/Debt/Bonds/">
	<!ENTITY fibo-sec-dbt-dbti "https://spec.edmcouncil.org/fibo/ontology/SEC/Debt/DebtInstruments/">
	<!ENTITY fibo-sec-dbt-ex "https://spec.edmcouncil.org/fibo/ontology/SEC/Debt/ExerciseConventions/">
	<!ENTITY fibo-sec-dbt-tstd "https://spec.edmcouncil.org/fibo/ontology/SEC/Debt/TradedShortTermDebt/">
	<!ENTITY fibo-sec-eq-eq "https://spec.edmcouncil.org/fibo/ontology/SEC/Equities/EquityInstruments/">
	<!ENTITY fibo-sec-sec-iss "https://spec.edmcouncil.org/fibo/ontology/SEC/Securities/SecuritiesIssuance/">
	<!ENTITY fibo-sec-sec-lst "https://spec.edmcouncil.org/fibo/ontology/SEC/Securities/SecuritiesListings/">
	<!ENTITY owl "http://www.w3.org/2002/07/owl#">
	<!ENTITY rdf "http://www.w3.org/1999/02/22-rdf-syntax-ns#">
	<!ENTITY rdfs "http://www.w3.org/2000/01/rdf-schema#">
	<!ENTITY skos "http://www.w3.org/2004/02/skos/core#">
	<!ENTITY sm "http://www.omg.org/techprocess/ab/SpecificationMetadata/">
	<!ENTITY xsd "http://www.w3.org/2001/XMLSchema#">
]>
<rdf:RDF xml:base="https://spec.edmcouncil.org/fibo/ontology/SEC/Debt/Bonds/"
	xmlns:dct="http://purl.org/dc/terms/"
	xmlns:fibo-be-ge-ge="https://spec.edmcouncil.org/fibo/ontology/BE/GovernmentEntities/GovernmentEntities/"
	xmlns:fibo-be-le-cb="https://spec.edmcouncil.org/fibo/ontology/BE/LegalEntities/CorporateBodies/"
	xmlns:fibo-be-le-lp="https://spec.edmcouncil.org/fibo/ontology/BE/LegalEntities/LegalPersons/"
	xmlns:fibo-fbc-dae-dbt="https://spec.edmcouncil.org/fibo/ontology/FBC/DebtAndEquities/Debt/"
	xmlns:fibo-fbc-dae-gty="https://spec.edmcouncil.org/fibo/ontology/FBC/DebtAndEquities/Guaranty/"
	xmlns:fibo-fbc-fi-fi="https://spec.edmcouncil.org/fibo/ontology/FBC/FinancialInstruments/FinancialInstruments/"
	xmlns:fibo-fbc-pas-fpas="https://spec.edmcouncil.org/fibo/ontology/FBC/ProductsAndServices/FinancialProductsAndServices/"
	xmlns:fibo-fnd-acc-cur="https://spec.edmcouncil.org/fibo/ontology/FND/Accounting/CurrencyAmount/"
	xmlns:fibo-fnd-agr-agr="https://spec.edmcouncil.org/fibo/ontology/FND/Agreements/Agreements/"
	xmlns:fibo-fnd-agr-ctr="https://spec.edmcouncil.org/fibo/ontology/FND/Agreements/Contracts/"
	xmlns:fibo-fnd-dt-bd="https://spec.edmcouncil.org/fibo/ontology/FND/DatesAndTimes/BusinessDates/"
	xmlns:fibo-fnd-dt-fd="https://spec.edmcouncil.org/fibo/ontology/FND/DatesAndTimes/FinancialDates/"
	xmlns:fibo-fnd-dt-oc="https://spec.edmcouncil.org/fibo/ontology/FND/DatesAndTimes/Occurrences/"
	xmlns:fibo-fnd-pas-psch="https://spec.edmcouncil.org/fibo/ontology/FND/ProductsAndServices/PaymentsAndSchedules/"
	xmlns:fibo-fnd-pty-rl="https://spec.edmcouncil.org/fibo/ontology/FND/Parties/Roles/"
	xmlns:fibo-fnd-rel-rel="https://spec.edmcouncil.org/fibo/ontology/FND/Relations/Relations/"
	xmlns:fibo-fnd-utl-alx="https://spec.edmcouncil.org/fibo/ontology/FND/Utilities/Analytics/"
	xmlns:fibo-fnd-utl-av="https://spec.edmcouncil.org/fibo/ontology/FND/Utilities/AnnotationVocabulary/"
	xmlns:fibo-fnd-utl-val="https://spec.edmcouncil.org/fibo/ontology/FND/Utilities/Values/"
	xmlns:fibo-ind-ei-ei="https://spec.edmcouncil.org/fibo/ontology/IND/EconomicIndicators/EconomicIndicators/"
	xmlns:fibo-ind-ind-ind="https://spec.edmcouncil.org/fibo/ontology/IND/Indicators/Indicators/"
	xmlns:fibo-ind-ir-ir="https://spec.edmcouncil.org/fibo/ontology/IND/InterestRates/InterestRates/"
	xmlns:fibo-sec-dbt-bnd="https://spec.edmcouncil.org/fibo/ontology/SEC/Debt/Bonds/"
	xmlns:fibo-sec-dbt-dbti="https://spec.edmcouncil.org/fibo/ontology/SEC/Debt/DebtInstruments/"
	xmlns:fibo-sec-dbt-ex="https://spec.edmcouncil.org/fibo/ontology/SEC/Debt/ExerciseConventions/"
	xmlns:fibo-sec-dbt-tstd="https://spec.edmcouncil.org/fibo/ontology/SEC/Debt/TradedShortTermDebt/"
	xmlns:fibo-sec-eq-eq="https://spec.edmcouncil.org/fibo/ontology/SEC/Equities/EquityInstruments/"
	xmlns:fibo-sec-sec-iss="https://spec.edmcouncil.org/fibo/ontology/SEC/Securities/SecuritiesIssuance/"
	xmlns:fibo-sec-sec-lst="https://spec.edmcouncil.org/fibo/ontology/SEC/Securities/SecuritiesListings/"
	xmlns:owl="http://www.w3.org/2002/07/owl#"
	xmlns:rdf="http://www.w3.org/1999/02/22-rdf-syntax-ns#"
	xmlns:rdfs="http://www.w3.org/2000/01/rdf-schema#"
	xmlns:skos="http://www.w3.org/2004/02/skos/core#"
	xmlns:sm="http://www.omg.org/techprocess/ab/SpecificationMetadata/"
	xmlns:xsd="http://www.w3.org/2001/XMLSchema#">
	
	<owl:Ontology rdf:about="https://spec.edmcouncil.org/fibo/ontology/SEC/Debt/Bonds/">
		<rdfs:label xml:lang="en">Bonds Ontology</rdfs:label>
		<dct:abstract>This ontology defines the basic concept of a bond and a number of bond variants including convertible and callable bonds. Medium term notes (MTNs) and debentures are also defined.</dct:abstract>
		<dct:license rdf:datatype="&xsd;anyURI">http://opensource.org/licenses/MIT</dct:license>
		<sm:contentLanguage rdf:resource="http://www.w3.org/standards/techs/owl#w3c_all"/>
		<sm:copyright>Copyright (c) 2016-2019 EDM Council, Inc.</sm:copyright>
		<sm:copyright>Copyright (c) 2018-2019 Object Management Group, Inc.</sm:copyright>
		<sm:dependsOn rdf:datatype="&xsd;anyURI">https://spec.edmcouncil.org/fibo/ontology/BE/</sm:dependsOn>
		<sm:dependsOn rdf:datatype="&xsd;anyURI">https://spec.edmcouncil.org/fibo/ontology/FBC/</sm:dependsOn>
		<sm:dependsOn rdf:datatype="&xsd;anyURI">https://spec.edmcouncil.org/fibo/ontology/FND/</sm:dependsOn>
		<sm:dependsOn rdf:datatype="&xsd;anyURI">https://spec.edmcouncil.org/fibo/ontology/IND/</sm:dependsOn>
		<sm:dependsOn rdf:datatype="&xsd;anyURI">https://spec.edmcouncil.org/fibo/ontology/SEC/Debt/DebtInstruments/</sm:dependsOn>
		<sm:dependsOn rdf:datatype="&xsd;anyURI">https://spec.edmcouncil.org/fibo/ontology/SEC/Debt/ExerciseConventions/</sm:dependsOn>
		<sm:dependsOn rdf:datatype="&xsd;anyURI">https://spec.edmcouncil.org/fibo/ontology/SEC/Debt/TradedShortTermDebt/</sm:dependsOn>
		<sm:dependsOn rdf:datatype="&xsd;anyURI">https://spec.edmcouncil.org/fibo/ontology/SEC/Equities/EquityInstruments/</sm:dependsOn>
		<sm:dependsOn rdf:datatype="&xsd;anyURI">https://spec.edmcouncil.org/fibo/ontology/SEC/Securities/SecuritiesIssuance/</sm:dependsOn>
		<sm:dependsOn rdf:datatype="&xsd;anyURI">https://spec.edmcouncil.org/fibo/ontology/SEC/Securities/SecuritiesListings/</sm:dependsOn>
		<sm:fileAbbreviation>fibo-sec-dbt-bnd</sm:fileAbbreviation>
		<sm:filename>Bonds.rdf</sm:filename>
		<owl:imports rdf:resource="https://spec.edmcouncil.org/fibo/ontology/BE/FunctionalEntities/FunctionalEntities/"/>
		<owl:imports rdf:resource="https://spec.edmcouncil.org/fibo/ontology/BE/GovernmentEntities/GovernmentEntities/"/>
		<owl:imports rdf:resource="https://spec.edmcouncil.org/fibo/ontology/BE/LegalEntities/CorporateBodies/"/>
		<owl:imports rdf:resource="https://spec.edmcouncil.org/fibo/ontology/BE/LegalEntities/LegalPersons/"/>
		<owl:imports rdf:resource="https://spec.edmcouncil.org/fibo/ontology/FBC/DebtAndEquities/Debt/"/>
		<owl:imports rdf:resource="https://spec.edmcouncil.org/fibo/ontology/FBC/DebtAndEquities/Guaranty/"/>
		<owl:imports rdf:resource="https://spec.edmcouncil.org/fibo/ontology/FBC/FinancialInstruments/FinancialInstruments/"/>
		<owl:imports rdf:resource="https://spec.edmcouncil.org/fibo/ontology/FBC/ProductsAndServices/FinancialProductsAndServices/"/>
		<owl:imports rdf:resource="https://spec.edmcouncil.org/fibo/ontology/FND/Accounting/CurrencyAmount/"/>
		<owl:imports rdf:resource="https://spec.edmcouncil.org/fibo/ontology/FND/Agreements/Agreements/"/>
		<owl:imports rdf:resource="https://spec.edmcouncil.org/fibo/ontology/FND/Agreements/Contracts/"/>
		<owl:imports rdf:resource="https://spec.edmcouncil.org/fibo/ontology/FND/DatesAndTimes/BusinessDates/"/>
		<owl:imports rdf:resource="https://spec.edmcouncil.org/fibo/ontology/FND/DatesAndTimes/FinancialDates/"/>
		<owl:imports rdf:resource="https://spec.edmcouncil.org/fibo/ontology/FND/DatesAndTimes/Occurrences/"/>
		<owl:imports rdf:resource="https://spec.edmcouncil.org/fibo/ontology/FND/Parties/Parties/"/>
		<owl:imports rdf:resource="https://spec.edmcouncil.org/fibo/ontology/FND/Parties/Roles/"/>
		<owl:imports rdf:resource="https://spec.edmcouncil.org/fibo/ontology/FND/ProductsAndServices/PaymentsAndSchedules/"/>
		<owl:imports rdf:resource="https://spec.edmcouncil.org/fibo/ontology/FND/Relations/Relations/"/>
		<owl:imports rdf:resource="https://spec.edmcouncil.org/fibo/ontology/FND/Utilities/Analytics/"/>
		<owl:imports rdf:resource="https://spec.edmcouncil.org/fibo/ontology/FND/Utilities/AnnotationVocabulary/"/>
		<owl:imports rdf:resource="https://spec.edmcouncil.org/fibo/ontology/FND/Utilities/Values/"/>
		<owl:imports rdf:resource="https://spec.edmcouncil.org/fibo/ontology/IND/EconomicIndicators/EconomicIndicators/"/>
		<owl:imports rdf:resource="https://spec.edmcouncil.org/fibo/ontology/IND/Indicators/Indicators/"/>
		<owl:imports rdf:resource="https://spec.edmcouncil.org/fibo/ontology/IND/InterestRates/InterestRates/"/>
		<owl:imports rdf:resource="https://spec.edmcouncil.org/fibo/ontology/SEC/Debt/DebtInstruments/"/>
		<owl:imports rdf:resource="https://spec.edmcouncil.org/fibo/ontology/SEC/Debt/ExerciseConventions/"/>
		<owl:imports rdf:resource="https://spec.edmcouncil.org/fibo/ontology/SEC/Debt/TradedShortTermDebt/"/>
		<owl:imports rdf:resource="https://spec.edmcouncil.org/fibo/ontology/SEC/Equities/EquityInstruments/"/>
		<owl:imports rdf:resource="https://spec.edmcouncil.org/fibo/ontology/SEC/Securities/SecuritiesIssuance/"/>
		<owl:imports rdf:resource="https://spec.edmcouncil.org/fibo/ontology/SEC/Securities/SecuritiesListings/"/>
		<owl:versionIRI rdf:resource="https://spec.edmcouncil.org/fibo/ontology/SEC/Debt/Bonds/"/>
		<fibo-fnd-utl-av:hasMaturityLevel rdf:resource="&fibo-fnd-utl-av;Provisional"/>
	</owl:Ontology>
	
	<owl:Class rdf:about="&fibo-sec-dbt-bnd;AmortizingBond">
		<rdfs:subClassOf rdf:resource="&fibo-sec-dbt-bnd;Bond"/>
		<rdfs:subClassOf>
			<owl:Restriction>
				<owl:onProperty rdf:resource="&fibo-sec-dbt-dbti;hasRepaymentTerms"/>
				<owl:someValuesFrom rdf:resource="&fibo-sec-dbt-bnd;BondAmortizationPaymentTerms"/>
			</owl:Restriction>
		</rdfs:subClassOf>
		<rdfs:label>amortizing bond</rdfs:label>
		<owl:disjointWith rdf:resource="&fibo-sec-dbt-bnd;BulletBond"/>
		<skos:definition>bond that regularly pays down the principal (face value) on the debt along with its interest expense over the life of the bond</skos:definition>
	</owl:Class>
	
	<owl:Class rdf:about="&fibo-sec-dbt-bnd;Bond">
		<rdfs:subClassOf rdf:resource="&fibo-sec-dbt-dbti;TradableDebtInstrument"/>
		<rdfs:subClassOf>
			<owl:Restriction>
				<owl:onProperty rdf:resource="&fibo-sec-dbt-dbti;hasInterestPaymentTerms"/>
				<owl:someValuesFrom rdf:resource="&fibo-sec-dbt-bnd;CouponPaymentTerms"/>
			</owl:Restriction>
		</rdfs:subClassOf>
		<rdfs:subClassOf>
			<owl:Restriction>
				<owl:onProperty rdf:resource="&fibo-sec-dbt-dbti;hasRepaymentTerms"/>
				<owl:someValuesFrom rdf:resource="&fibo-sec-dbt-bnd;BondPrincipalRepaymentTerms"/>
			</owl:Restriction>
		</rdfs:subClassOf>
		<rdfs:label>bond</rdfs:label>
		<skos:definition>fixed-income instrument in which the issuer owes the holders a debt and, depending on the terms of the bond, is obliged to pay interest (the coupon) and/or to repay the principal at maturity</skos:definition>
	</owl:Class>
	
	<owl:Class rdf:about="&fibo-sec-dbt-bnd;BondAmortizationPaymentTerms">
		<rdfs:subClassOf rdf:resource="&fibo-sec-dbt-bnd;BondPrincipalRepaymentTerms"/>
		<rdfs:label xml:lang="en">bond amortization payment terms</rdfs:label>
		<owl:disjointWith rdf:resource="&fibo-sec-dbt-bnd;BulletPrincipalRepaymentTerms"/>
	</owl:Class>
	
	<owl:Class rdf:about="&fibo-sec-dbt-bnd;BondConversionTerms">
		<rdfs:subClassOf rdf:resource="&fibo-sec-dbt-dbti;TradableDebtInstrumentRedemptionProvision"/>
		<rdfs:subClassOf rdf:resource="&fibo-sec-sec-iss;ConversionTerms"/>
		<rdfs:subClassOf>
			<owl:Restriction>
				<owl:onProperty rdf:resource="&fibo-sec-sec-iss;specifiesConversionInto"/>
				<owl:someValuesFrom rdf:resource="&fibo-sec-eq-eq;PubliclyTradedShare"/>
			</owl:Restriction>
		</rdfs:subClassOf>
		<rdfs:label>bond conversion terms</rdfs:label>
		<skos:definition>terms indicating when a convertible bond can be converted to another security (usually a publicly traded share issued by of the same issuer).</skos:definition>
	</owl:Class>
	
	<owl:Class rdf:about="&fibo-sec-dbt-bnd;BondCoupon">
		<rdfs:subClassOf rdf:resource="&fibo-fnd-acc-cur;InterestRate"/>
		<rdfs:label>bond coupon</rdfs:label>
		<skos:definition>interest rate on a debt security that the issuer promises to pay to the holder until maturity, expressed as an annual percentage of the face value</skos:definition>
		<fibo-fnd-utl-av:synonym>coupon percent rate</fibo-fnd-utl-av:synonym>
		<fibo-fnd-utl-av:synonym>coupon rate</fibo-fnd-utl-av:synonym>
		<fibo-fnd-utl-av:synonym>nominal yield</fibo-fnd-utl-av:synonym>
	</owl:Class>
	
	<owl:Class rdf:about="&fibo-sec-dbt-bnd;BondInsurance">
		<rdfs:subClassOf rdf:resource="&fibo-fbc-dae-gty;InsurancePolicy"/>
		<rdfs:label>bond insurance</rdfs:label>
		<skos:definition>insurance policy that a bond issuer purchases that guarantees the repayment of the principal and all associated interest payments to the bondholders in the event of default</skos:definition>
		<skos:editorialNote>From April 21 Review: For cash CDOs: External e.g. Bond insurance that is bought from a 3rd party. NB Does not apply to synthetics. Also CDOs may have internal crefit enhancement instead. See main diagram note on this.</skos:editorialNote>
	</owl:Class>
	
	<owl:Class rdf:about="&fibo-sec-dbt-bnd;BondListing">
		<rdfs:subClassOf rdf:resource="&fibo-sec-sec-lst;SecurityListing"/>
		<rdfs:label>bond listing</rdfs:label>
	</owl:Class>
	
	<owl:Class rdf:about="&fibo-sec-dbt-bnd;BondMaturityRegistrar">
		<rdfs:subClassOf rdf:resource="&fibo-fbc-pas-fpas;LegalAgent"/>
		<rdfs:subClassOf rdf:resource="&fibo-fnd-agr-ctr;ContractThirdParty"/>
		<rdfs:label>bond maturity registrar</rdfs:label>
		<skos:definition>person or entity responsible for maintaining records on behalf of the issuer that identify the owners of a registered bond issue</skos:definition>
		<fibo-fnd-utl-av:explanatoryNote>The trustee under a bond contract often also acts as registrar.</fibo-fnd-utl-av:explanatoryNote>
	</owl:Class>
	
	<owl:Class rdf:about="&fibo-sec-dbt-bnd;BondPrincipalRepaymentTerms">
		<rdfs:subClassOf rdf:resource="&fibo-sec-dbt-dbti;TradableDebtInstrumentRedemptionProvision"/>
		<rdfs:label>bond principal repayment terms</rdfs:label>
		<owl:disjointWith rdf:resource="&fibo-sec-dbt-dbti;CallFeature"/>
		<skos:definition>terms for the repayment of the principal on a bond security</skos:definition>
	</owl:Class>
	
	<owl:Class rdf:about="&fibo-sec-dbt-bnd;BondVariableCoupon">
		<rdfs:subClassOf rdf:resource="&fibo-fbc-dae-dbt;VariableInterestRate"/>
		<rdfs:subClassOf rdf:resource="&fibo-sec-dbt-bnd;BondCoupon"/>
		<rdfs:label>bond variable coupon</rdfs:label>
		<skos:definition>bond coupon that is defined as a variable interest rate</skos:definition>
	</owl:Class>
	
	<owl:Class rdf:about="&fibo-sec-dbt-bnd;BondWithMandatorySinkingFund">
		<rdfs:subClassOf rdf:resource="&fibo-sec-dbt-bnd;AmortizingBond"/>
		<rdfs:subClassOf>
			<owl:Restriction>
				<owl:onProperty rdf:resource="&fibo-fnd-agr-ctr;hasContractualElement"/>
				<owl:someValuesFrom rdf:resource="&fibo-sec-dbt-bnd;MandatorySinkingFundTerms"/>
			</owl:Restriction>
		</rdfs:subClassOf>
		<rdfs:label>bond with mandatory sinking fund</rdfs:label>
		<skos:definition>bond in which amortization is via a sinking fund, the details of which are specified in the terms of the bond</skos:definition>
	</owl:Class>
	
	<owl:Class rdf:about="&fibo-sec-dbt-bnd;BondWithPartialCall">
		<rdfs:subClassOf rdf:resource="&fibo-sec-dbt-bnd;CallableBond"/>
		<rdfs:subClassOf>
			<owl:Restriction>
				<owl:onProperty rdf:resource="&fibo-sec-dbt-dbti;hasCallFeature"/>
				<owl:someValuesFrom rdf:resource="&fibo-sec-dbt-bnd;PartialCallFeature"/>
			</owl:Restriction>
		</rdfs:subClassOf>
		<rdfs:label>bond with partial call</rdfs:label>
		<skos:definition>bond with a feature whereby the issue can be partially called for amounts that are at the discretion of the issuer</skos:definition>
	</owl:Class>
	
	<owl:Class rdf:about="&fibo-sec-dbt-bnd;BondWithPublishedSinkingFund">
		<rdfs:subClassOf rdf:resource="&fibo-sec-dbt-bnd;AmortizingBond"/>
		<rdfs:label>bond with published sinking fund</rdfs:label>
		<skos:definition>bond whereby amortization is via a known and published schedule</skos:definition>
	</owl:Class>
	
	<owl:Class rdf:about="&fibo-sec-dbt-bnd;BondWithWarrant">
		<rdfs:subClassOf rdf:resource="&fibo-sec-dbt-dbti;DebtOffering"/>
		<rdfs:label>bond with warrant</rdfs:label>
		<skos:definition>bond issue whereby the issue includes a warrant</skos:definition>
		<skos:editorialNote>This need not be any specific type of bond. This is NOT a kind of Bond Contract but a kind of Issue Offer, and is modeled as such, in the Issuance Terms section of the model. This class of contract is retained in the model for now in order to provide traceability with the CFI term for &quot;Bond With Warrant&quot; only.</skos:editorialNote>
	</owl:Class>
	
	<owl:Class rdf:about="&fibo-sec-dbt-bnd;BuildAmericaBond">
		<rdfs:subClassOf rdf:resource="&fibo-sec-dbt-bnd;MunicipalBond"/>
		<rdfs:label>Build America bond</rdfs:label>
		<skos:definition>taxable municipal bond issued through December 31, 2010 under the American Recovery and Reinvestment Act of 2009 (ARRA)</skos:definition>
		<fibo-fnd-utl-av:explanatoryNote>BABs may be direct pay subsidy bonds or tax credit bonds.</fibo-fnd-utl-av:explanatoryNote>
	</owl:Class>
	
	<owl:Class rdf:about="&fibo-sec-dbt-bnd;BulletBond">
		<rdfs:subClassOf rdf:resource="&fibo-sec-dbt-bnd;Bond"/>
		<rdfs:subClassOf>
			<owl:Restriction>
				<owl:onProperty rdf:resource="&fibo-sec-dbt-dbti;hasRepaymentTerms"/>
				<owl:someValuesFrom rdf:resource="&fibo-sec-dbt-bnd;BulletPrincipalRepaymentTerms"/>
			</owl:Restriction>
		</rdfs:subClassOf>
		<rdfs:label>bullet bond</rdfs:label>
		<owl:disjointWith rdf:resource="&fibo-sec-dbt-bnd;AmortizingBond"/>
		<owl:disjointWith rdf:resource="&fibo-sec-dbt-bnd;CallableBond"/>
		<skos:definition>bond whose entire principal value is paid on the maturity date, rather than amortized over its lifetime</skos:definition>
	</owl:Class>
	
	<owl:Class rdf:about="&fibo-sec-dbt-bnd;BulletPrincipalRepaymentTerms">
		<rdfs:subClassOf rdf:resource="&fibo-sec-dbt-bnd;BondPrincipalRepaymentTerms"/>
		<rdfs:label>bond bullet principal repayment terms</rdfs:label>
		<skos:definition>terms for repayment of the principal for a bond as a single payment covering the whole principal amount</skos:definition>
	</owl:Class>
	
	<owl:Class rdf:about="&fibo-sec-dbt-bnd;CallableBond">
		<rdfs:subClassOf rdf:resource="&fibo-sec-dbt-bnd;Bond"/>
		<rdfs:subClassOf>
			<owl:Restriction>
				<owl:onProperty rdf:resource="&fibo-sec-dbt-dbti;isCallable"/>
				<owl:hasValue rdf:datatype="&xsd;boolean">true</owl:hasValue>
			</owl:Restriction>
		</rdfs:subClassOf>
		<rdfs:subClassOf>
			<owl:Restriction>
				<owl:onProperty rdf:resource="&fibo-sec-dbt-bnd;hasExtraordinaryRedemptionProvision"/>
				<owl:onClass rdf:resource="&fibo-sec-dbt-bnd;ExtraordinaryRedemptionProvision"/>
				<owl:maxQualifiedCardinality rdf:datatype="&xsd;nonNegativeInteger">1</owl:maxQualifiedCardinality>
			</owl:Restriction>
		</rdfs:subClassOf>
		<rdfs:subClassOf>
			<owl:Restriction>
				<owl:onProperty rdf:resource="&fibo-sec-dbt-dbti;hasCallFeature"/>
				<owl:someValuesFrom rdf:resource="&fibo-sec-dbt-dbti;CallFeature"/>
			</owl:Restriction>
		</rdfs:subClassOf>
		<rdfs:label>callable bond</rdfs:label>
		<skos:definition>a bond giving the issuer the right to buy it back at the call price after the call protection period</skos:definition>
	</owl:Class>
	
	<owl:Class rdf:about="&fibo-sec-dbt-bnd;CallableConvertibleBond">
		<rdfs:subClassOf rdf:resource="&fibo-sec-dbt-bnd;CallableBond"/>
		<rdfs:subClassOf rdf:resource="&fibo-sec-dbt-bnd;ConvertibleBond"/>
		<rdfs:label>callable convertible bond</rdfs:label>
		<skos:definition>a convertible bond that is also callable</skos:definition>
	</owl:Class>
	
	<owl:Class rdf:about="&fibo-sec-dbt-bnd;CertificateOfObligation">
		<rdfs:subClassOf rdf:resource="&fibo-sec-dbt-bnd;MunicipalSecurity"/>
		<rdfs:label>certificate of obligation</rdfs:label>
		<skos:definition>a municipal security available to governing councils in case of emergency, such as a natural disaster, that needs immediate action without time for voter referendum</skos:definition>
		<fibo-fnd-utl-av:explanatoryNote>For example, when a hurricane destroys the police and emergency services building, there is no time to go through the process of voter referendum. The local council must be able to borrow the money to set up provisional buildings and necessary equipment for police and emergency services so that the community is served in continuity.</fibo-fnd-utl-av:explanatoryNote>
	</owl:Class>
	
	<owl:Class rdf:about="&fibo-sec-dbt-bnd;CertificateOfParticipation">
		<rdfs:subClassOf rdf:resource="&fibo-sec-dbt-bnd;MunicipalSecurity"/>
		<rdfs:label>certificate of participation</rdfs:label>
		<skos:definition>a municipal security evidencing a pro rata share in a specific pledged revenue stream, usually lease payments by the issuer that are typically subject to annual appropriation</skos:definition>
		<fibo-fnd-utl-av:explanatoryNote>The certificate generally entitles the holder to receive a share, or participation, in the payments from a particular project. The payments are passed through the lessor to the certificate holders. The lessor typically assigns the lease and the payments to a trustee, which then distributes the payments to the certificate holders.</fibo-fnd-utl-av:explanatoryNote>
	</owl:Class>
	
	<owl:Class rdf:about="&fibo-sec-dbt-bnd;ClawBackCall">
		<rdfs:subClassOf rdf:resource="&fibo-sec-dbt-bnd;EntireCall"/>
		<rdfs:label>claw back call</rdfs:label>
	</owl:Class>
	
	<owl:Class rdf:about="&fibo-sec-dbt-bnd;ConditionalCouponTerms">
		<rdfs:subClassOf rdf:resource="&fibo-sec-dbt-bnd;CouponPaymentTerms"/>
		<rdfs:subClassOf>
			<owl:Restriction>
				<owl:onProperty rdf:resource="&fibo-fnd-rel-rel;comprises"/>
				<owl:someValuesFrom rdf:resource="&fibo-sec-dbt-bnd;CouponConditionalTerm"/>
			</owl:Restriction>
		</rdfs:subClassOf>
		<rdfs:label>conditional coupon terms</rdfs:label>
		<owl:disjointWith rdf:resource="&fibo-sec-dbt-bnd;SingleCouponTerms"/>
		<owl:disjointWith rdf:resource="&fibo-sec-dbt-bnd;SteppedCouponTerms"/>
	</owl:Class>
	
	<owl:Class rdf:about="&fibo-sec-dbt-bnd;ControlledAmortizationBond">
		<rdfs:subClassOf rdf:resource="&fibo-sec-dbt-bnd;AmortizingBond"/>
		<rdfs:subClassOf>
			<owl:Restriction>
				<owl:onProperty rdf:resource="&fibo-sec-dbt-dbti;hasRepaymentTerms"/>
				<owl:someValuesFrom rdf:resource="&fibo-sec-dbt-bnd;ControlledAmortizationStructure"/>
			</owl:Restriction>
		</rdfs:subClassOf>
		<rdfs:label>controlled amortization bond</rdfs:label>
		<skos:definition>bond that is securitized using a controlled amortization structure</skos:definition>
		<fibo-fnd-utl-av:adaptedFrom>http://www.investinginbonds.com/learnmore.asp?catid=11&amp;subcatid=57&amp;id=15</fibo-fnd-utl-av:adaptedFrom>
		<fibo-fnd-utl-av:explanatoryNote>Revolving debt (primarily credit card receivables, but also HELOCs, trade receivables, dealer floor-plan loans and some leases) may be securitized using a controlled amortization structure. This is a method of providing investors with a relatively predictable repayment schedule, even though the underlying assets are nonamortizing. Controlled-amortization ABS resemble corporate bonds with a sinking fund. After a predetermined “revolving” period during which only interest payments are made, these securities attempt to return principal to investors in a series of defined periodic payments that usually occur over less than a year. A risk inherent in this kind of ABS is an early amortization event. (See “Early-Amortization Risk,” on page 20.)</fibo-fnd-utl-av:explanatoryNote>
	</owl:Class>
	
	<owl:Class rdf:about="&fibo-sec-dbt-bnd;ControlledAmortizationStructure">
		<rdfs:subClassOf rdf:resource="&fibo-sec-dbt-bnd;BondAmortizationPaymentTerms"/>
		<rdfs:label>controlled amortization structure</rdfs:label>
		<skos:definition>method of providing investors with a relatively predictable repayment schedule, even though the underlying assets are nonamortizing</skos:definition>
	</owl:Class>
	
	<owl:Class rdf:about="&fibo-sec-dbt-bnd;ConvertibleBond">
		<rdfs:subClassOf rdf:resource="&fibo-sec-dbt-bnd;Bond"/>
		<rdfs:subClassOf rdf:resource="&fibo-sec-sec-iss;ConvertibleSecurity"/>
		<rdfs:subClassOf>
			<owl:Restriction>
				<owl:onProperty rdf:resource="&fibo-fnd-agr-ctr;hasContractualElement"/>
				<owl:someValuesFrom rdf:resource="&fibo-sec-dbt-bnd;BondConversionTerms"/>
			</owl:Restriction>
		</rdfs:subClassOf>
		<rdfs:label>convertible bond</rdfs:label>
		<skos:definition>bond that converts to an equity instrument on maturity</skos:definition>
		<skos:editorialNote>There are different types based on the available exercise windows and facts thereof. Notes from CAE review on 7 July 2011 1. Convertible - meaning a convertible Bond whi ch converts into an Equity later in its life 2. Contingent Conversion (of what? - of a Debt. So it&apos;s a kind of Convertible) - if the share price reaches a particular threshold on a particular time window = COCO. - this is a debt instrument. you get the share when it reaches that price threshold. There are time windows (like traditional options instruments - i.e. Bermudan?) - is it mandatory to take a share it&apos;s mandatory - like a digital options which are also not really optional . The distinction is the time window.</skos:editorialNote>
	</owl:Class>
	
	<owl:Class rdf:about="&fibo-sec-dbt-bnd;CorporateBond">
		<rdfs:subClassOf rdf:resource="&fibo-sec-dbt-bnd;Bond"/>
		<rdfs:subClassOf>
			<owl:Restriction>
				<owl:onProperty rdf:resource="&fibo-fnd-rel-rel;isIssuedBy"/>
				<owl:someValuesFrom>
					<owl:Restriction>
						<owl:onProperty rdf:resource="&fibo-fnd-pty-rl;isPlayedBy"/>
						<owl:someValuesFrom rdf:resource="&fibo-be-le-lp;LegalEntity"/>
					</owl:Restriction>
				</owl:someValuesFrom>
			</owl:Restriction>
		</rdfs:subClassOf>
		<rdfs:label>corporate bond</rdfs:label>
		<owl:disjointWith rdf:resource="&fibo-sec-dbt-bnd;GovernmentBond"/>
		<owl:disjointWith rdf:resource="&fibo-sec-dbt-bnd;MunicipalBond"/>
		<skos:definition>debt security issued by a corporation, as opposed to those issued by a government or municipality</skos:definition>
		<skos:editorialNote>Added by extension from CFI Municipal. If there are Municipal Bonds in the classification hierarchy then Corporate and Government should also be included.</skos:editorialNote>
	</owl:Class>
	
	<owl:Class rdf:about="&fibo-sec-dbt-bnd;CouponConditionalTerm">
		<rdfs:subClassOf rdf:resource="&fibo-sec-dbt-bnd;CouponPaymentTerms"/>
		<rdfs:label>coupon conditional term</rdfs:label>
		<skos:definition>term in the conditional coupon terms that matches one set of coupon terms (fixed rate or variable coupon) with one condition</skos:definition>
	</owl:Class>
	
	<owl:Class rdf:about="&fibo-sec-dbt-bnd;CouponPayment">
		<rdfs:subClassOf rdf:resource="&fibo-fnd-pas-psch;PaymentEvent"/>
		<rdfs:label>coupon payment</rdfs:label>
		<skos:definition>payment event involving an interest payment on a bond (i.e., a coupon payment)</skos:definition>
	</owl:Class>
	
	<owl:Class rdf:about="&fibo-sec-dbt-bnd;CouponPaymentTerms">
		<rdfs:subClassOf rdf:resource="&fibo-fbc-dae-dbt;InterestPaymentTerms"/>
		<rdfs:subClassOf>
			<owl:Restriction>
				<owl:onProperty rdf:resource="&fibo-fbc-dae-dbt;hasInterestRate"/>
				<owl:someValuesFrom rdf:resource="&fibo-sec-dbt-bnd;BondCoupon"/>
			</owl:Restriction>
		</rdfs:subClassOf>
		<rdfs:subClassOf>
			<owl:Restriction>
				<owl:onProperty rdf:resource="&fibo-fnd-dt-fd;hasSchedule"/>
				<owl:someValuesFrom rdf:resource="&fibo-sec-dbt-bnd;CouponSchedule"/>
			</owl:Restriction>
		</rdfs:subClassOf>
		<rdfs:subClassOf>
			<owl:Restriction>
				<owl:onProperty rdf:resource="&fibo-sec-dbt-bnd;hasCouponCurrency"/>
				<owl:someValuesFrom rdf:resource="&fibo-fnd-acc-cur;Currency"/>
			</owl:Restriction>
		</rdfs:subClassOf>
		<rdfs:label>coupon payment terms</rdfs:label>
		<skos:definition xml:lang="en">terms for payment of interest on a bond</skos:definition>
	</owl:Class>
	
	<owl:Class rdf:about="&fibo-sec-dbt-bnd;CouponSchedule">
		<rdfs:subClassOf rdf:resource="&fibo-fnd-pas-psch;PaymentSchedule"/>
		<rdfs:subClassOf>
			<owl:Restriction>
				<owl:onProperty rdf:resource="&fibo-fnd-rel-rel;comprises"/>
				<owl:someValuesFrom rdf:resource="&fibo-sec-dbt-bnd;CouponPayment"/>
			</owl:Restriction>
		</rdfs:subClassOf>
		<rdfs:label>coupon schedule</rdfs:label>
		<skos:definition>payment schedule that consists of interest payments on a bond</skos:definition>
	</owl:Class>
	
	<owl:Class rdf:about="&fibo-sec-dbt-bnd;DanishBorrowerCall">
		<rdfs:subClassOf rdf:resource="&fibo-sec-dbt-dbti;CallEvent"/>
		<rdfs:label>danish borrower call</rdfs:label>
	</owl:Class>
	
	<owl:Class rdf:about="&fibo-sec-dbt-bnd;Debenture">
		<rdfs:subClassOf rdf:resource="&fibo-sec-dbt-bnd;Bond"/>
		<rdfs:subClassOf>
			<owl:Restriction>
				<owl:onProperty rdf:resource="&fibo-fnd-agr-ctr;hasContractualElement"/>
				<owl:onClass rdf:resource="&fibo-sec-dbt-bnd;DebentureSecuritizationConditions"/>
				<owl:maxQualifiedCardinality rdf:datatype="&xsd;nonNegativeInteger">1</owl:maxQualifiedCardinality>
			</owl:Restriction>
		</rdfs:subClassOf>
		<rdfs:label>debenture</rdfs:label>
		<skos:definition>general debt obligation backed only by the integrity of the borrower</skos:definition>
		<fibo-fnd-utl-av:explanatoryNote>Debentures are backed only by the general creditworthiness and reputation of the issuer. Both corporations and governments frequently issue this type of bond in order to secure capital. Like other types of bonds, debentures are documented in an indenture. May be jurisdiction-specific.</fibo-fnd-utl-av:explanatoryNote>
		<fibo-fnd-utl-av:explanatoryNote>From Wikipedia: In law, a debenture is a document which either creates a debt or acknowledges it. It is a medium to long-term borrowing facility created by a company. Where repayment is secured by a charge over land, the document is called a &apos;mortgage&apos;. Where repayment is secured by a charge other assets of the company, the document is called a &apos;debenture&apos;. Where no security is involved, the document is called a note or &apos;unsecured deposit note&apos;. There are two types of debentures: 1. Convertible Debentures, which are convertible bonds or bonds that can be converted into equity shares of the issuing company after a predetermined period of time. &quot;Convertibility&quot; is a feature that corporations may add to the bonds they issue in order to make them more attractive to buyers. In other words, it is a special feature that a corporate bond may carry. As a result of the advantage a buyer gets from the ability to convert, convertible bonds typically have lower interest rates than non-convertible corporate bonds. 2. Non-Convertible Debentures, which are simply regular debentures, cannot be converted into equity shares of the liable company. They are debentures without the convertibility feature attached to them. As a result, they usually carry higher interest rates than their convertible counterparts.</fibo-fnd-utl-av:explanatoryNote>
	</owl:Class>
	
	<owl:Class rdf:about="&fibo-sec-dbt-bnd;DebentureSecuritizationConditions">
		<rdfs:subClassOf rdf:resource="&fibo-fnd-agr-ctr;ContractualCommitment"/>
		<rdfs:label>debenture securitization conditions</rdfs:label>
		<skos:definition>terms, if any, by which a debenture is secured; may include a description of the properties by which it is secured, and or any priority claims related to that</skos:definition>
		<skos:editorialNote>A debenture is usually unsecured in the sense that there are no liens or pledges on specific assets. It is however, secured by all properties not otherwise pledged. From Wikipedia A debenture (also called a note) is an unsecured corporate bond or a corporate bond that does not have a certain line of income or piece of property or equipment to guarantee repayment of principal upon the bond&apos;s maturity. Debentures are long-term debt instrument used by large companies to obtain funds. Where securities are offered, loan stocks or bonds are termed &apos;debentures&apos; in the UK or &apos;mortgage bonds&apos; in the US. Summary: Therefore they are unsecured in the sense of not having a particular cash flow allocated to them, but they are therefore secured by some other asset.</skos:editorialNote>
	</owl:Class>
	
	<owl:Class rdf:about="&fibo-sec-dbt-bnd;EntireCall">
		<rdfs:subClassOf rdf:resource="&fibo-sec-dbt-dbti;CallEvent"/>
		<rdfs:label>entire call</rdfs:label>
	</owl:Class>
	
	<owl:Class rdf:about="&fibo-sec-dbt-bnd;EntireOrPartialCallChoice">
		<rdfs:label>entire or partial call choice</rdfs:label>
	</owl:Class>
	
	<owl:Class rdf:about="&fibo-sec-dbt-bnd;EquityLinkedBond">
		<rdfs:subClassOf rdf:resource="&fibo-sec-dbt-bnd;VariableCouponBond"/>
		<rdfs:label>equity linked bond</rdfs:label>
		<skos:definition>bond based on the return on an equity over time, i.e. the price and dividend payments or the total return (similar to total return swaps)</skos:definition>
	</owl:Class>
	
	<owl:Class rdf:about="&fibo-sec-dbt-bnd;ExtraordinaryRedemptionProvision">
		<rdfs:subClassOf rdf:resource="&fibo-sec-dbt-dbti;CallFeature"/>
		<rdfs:label>extraordinary redemption provision</rdfs:label>
		<owl:disjointWith rdf:resource="&fibo-sec-dbt-bnd;RegularCall"/>
		<skos:definition>provision that gives a bond issuer the right to call its bonds due to an unusual one-time occurrence, as specified in the offering statement</skos:definition>
		<fibo-fnd-utl-av:explanatoryNote>Such redemptions may occur when bond proceeds are not spent according to schedule; when bond proceeds are used in a way that makes nontaxable bond interest taxable; or when a catastrophe destroys the project being financed, among other reasons.</fibo-fnd-utl-av:explanatoryNote>
	</owl:Class>
	
	<owl:Class rdf:about="&fibo-sec-dbt-bnd;FirstRegularCouponDate">
		<rdfs:subClassOf rdf:resource="&fibo-fnd-dt-fd;ExplicitDate"/>
		<rdfs:label>first regular coupon date</rdfs:label>
		<skos:definition>scheduled date for the first regular coupon payment, in a regular repeating series of coupon periods, after any non standard (long or short) first coupon period in the schedule</skos:definition>
	</owl:Class>
	
	<owl:Class rdf:about="&fibo-sec-dbt-bnd;FixedCouponBond">
		<rdfs:subClassOf rdf:resource="&fibo-sec-dbt-bnd;Bond"/>
		<rdfs:subClassOf>
			<owl:Restriction>
				<owl:onProperty rdf:resource="&fibo-sec-dbt-dbti;hasInterestPaymentTerms"/>
				<owl:someValuesFrom rdf:resource="&fibo-sec-dbt-bnd;FixedCouponTerms"/>
			</owl:Restriction>
		</rdfs:subClassOf>
		<rdfs:label>fixed coupon bond</rdfs:label>
		<owl:disjointWith rdf:resource="&fibo-sec-dbt-bnd;VariableCouponBond"/>
		<skos:definition>a bond that pays a fixed rate of interest at regular intervals</skos:definition>
	</owl:Class>
	
	<owl:Class rdf:about="&fibo-sec-dbt-bnd;FixedCouponTerms">
		<rdfs:subClassOf rdf:resource="&fibo-sec-dbt-bnd;CouponPaymentTerms"/>
		<rdfs:subClassOf>
			<owl:Restriction>
				<owl:onProperty rdf:resource="&fibo-fbc-dae-dbt;hasInterestRate"/>
				<owl:someValuesFrom rdf:resource="&fibo-fbc-dae-dbt;FixedInterestRate"/>
			</owl:Restriction>
		</rdfs:subClassOf>
		<rdfs:label>fixed coupon terms</rdfs:label>
		<owl:disjointWith rdf:resource="&fibo-sec-dbt-bnd;VariableCouponTerms"/>
		<skos:definition>terms for payment of interest on a bond with a fixed interest rate</skos:definition>
	</owl:Class>
	
	<owl:Class rdf:about="&fibo-sec-dbt-bnd;FloatingRateNote">
		<rdfs:subClassOf rdf:resource="&fibo-sec-dbt-bnd;VariableCouponBond"/>
		<rdfs:subClassOf>
			<owl:Restriction>
				<owl:onProperty rdf:resource="&fibo-fbc-dae-dbt;hasInterestRate"/>
				<owl:someValuesFrom rdf:resource="&fibo-sec-dbt-bnd;FloatingRateNoteCoupon"/>
			</owl:Restriction>
		</rdfs:subClassOf>
		<rdfs:subClassOf>
			<owl:Restriction>
				<owl:onProperty rdf:resource="&fibo-sec-dbt-dbti;hasInterestPaymentTerms"/>
				<owl:someValuesFrom rdf:resource="&fibo-sec-dbt-bnd;FloatingRateNoteTerms"/>
			</owl:Restriction>
		</rdfs:subClassOf>
		<rdfs:label>floating rate note</rdfs:label>
		<skos:definition>bond with a variable interest rate based on a published reference interest rate</skos:definition>
		<fibo-fnd-utl-av:explanatoryNote>The adjustments to the interest rate (coupon) are made periodically, usually on a quarterly or monthly basis, and are tied to a certain money-market index. Also known as a &quot;floater&quot;. For example six months USD LIBOR + 0.20%.</fibo-fnd-utl-av:explanatoryNote>
	</owl:Class>
	
	<owl:Class rdf:about="&fibo-sec-dbt-bnd;FloatingRateNoteCoupon">
		<rdfs:subClassOf rdf:resource="&fibo-sec-dbt-bnd;BondVariableCoupon"/>
		<rdfs:label>floating rate note coupon</rdfs:label>
		<owl:disjointWith rdf:resource="&fibo-sec-dbt-bnd;IndexLinkedCoupon"/>
		<owl:disjointWith rdf:resource="&fibo-sec-dbt-bnd;InflationBondVariableCoupon"/>
		<owl:disjointWith rdf:resource="&fibo-sec-dbt-bnd;WACBondCoupon"/>
		<skos:definition>Mechanism whereby an investor receives income from interest payments, which are usually made periodically. These are for a variable amount based on a specified Interest rate.</skos:definition>
	</owl:Class>
	
	<owl:Class rdf:about="&fibo-sec-dbt-bnd;FloatingRateNoteTerms">
		<rdfs:subClassOf rdf:resource="&fibo-sec-dbt-bnd;VariableCouponTerms"/>
		<rdfs:subClassOf>
			<owl:Restriction>
				<owl:onProperty rdf:resource="&fibo-fbc-dae-dbt;isBasedOn"/>
				<owl:someValuesFrom rdf:resource="&fibo-ind-ir-ir;ReferenceInterestRate"/>
			</owl:Restriction>
		</rdfs:subClassOf>
		<rdfs:label>floating rate note terms</rdfs:label>
		<owl:disjointWith rdf:resource="&fibo-sec-dbt-bnd;IndexLinkedCouponTerms"/>
		<owl:disjointWith rdf:resource="&fibo-sec-dbt-bnd;InflationBondVariableCouponTerms"/>
		<skos:definition>terms specifying interest payments and dates for a floating rate note (FRN)</skos:definition>
	</owl:Class>
	
	<owl:Class rdf:about="&fibo-sec-dbt-bnd;FullFaithAndCreditBond">
		<rdfs:subClassOf rdf:resource="&fibo-sec-dbt-bnd;Bond"/>
		<rdfs:label>full faith and credit bond</rdfs:label>
		<skos:definition>bond secured by an unconditional promise to pay by another entity</skos:definition>
		<fibo-fnd-utl-av:explanatoryNote>Full faith and credit bonds are typically backed by a government entity and are considered low risk. The full faith and credit commitment is typically employed by a government to help lower the borrowing costs of a smaller, less stable government or a government-sponsored agency.</fibo-fnd-utl-av:explanatoryNote>
	</owl:Class>
	
	<owl:Class rdf:about="&fibo-sec-dbt-bnd;FullyAmortizingBond">
		<rdfs:subClassOf rdf:resource="&fibo-sec-dbt-bnd;AmortizingBond"/>
		<rdfs:label>fully amortizing bond</rdfs:label>
		<skos:definition>amortizing bond that returns principal to investors over the life of the security</skos:definition>
		<fibo-fnd-utl-av:definitionOrigin>http://www.investinginbonds.com/learnmore.asp?catid=11&amp;subcatid=57&amp;id=15</fibo-fnd-utl-av:definitionOrigin>
		<fibo-fnd-utl-av:explanatoryNote>Fully amortizing bonds are designed to closely reflect the full repayment of the underlying loans through scheduled interest and principal payments.</fibo-fnd-utl-av:explanatoryNote>
		<fibo-fnd-utl-av:explanatoryNote>These are typically backed by HELs, auto loans, manufactured-housing contracts and other fully amortizing assets. Prepayment risk is a key consideration with such ABS, although the rate of prepayment may vary considerably by the type of underlying asset.</fibo-fnd-utl-av:explanatoryNote>
	</owl:Class>
	
	<owl:Class rdf:about="&fibo-sec-dbt-bnd;GeneralObligationMunicipalBond">
		<rdfs:subClassOf rdf:resource="&fibo-sec-dbt-bnd;FullFaithAndCreditBond"/>
		<rdfs:subClassOf rdf:resource="&fibo-sec-dbt-bnd;MunicipalBond"/>
		<rdfs:label>general obligation municipal bond</rdfs:label>
		<owl:disjointWith rdf:resource="&fibo-sec-dbt-bnd;RevenueBond"/>
		<skos:definition>a full faith and credit municipal bond that is not backed by revenue from a specific project</skos:definition>
		<fibo-fnd-utl-av:abbreviation>GO</fibo-fnd-utl-av:abbreviation>
		<fibo-fnd-utl-av:explanatoryNote>A general obligation bond is secured by an issuing government&apos;s pledge to use all available resources - even tax revenues - to repay holders of the bond.</fibo-fnd-utl-av:explanatoryNote>
	</owl:Class>
	
	<owl:Class rdf:about="&fibo-sec-dbt-bnd;GovernmentBond">
		<rdfs:subClassOf rdf:resource="&fibo-sec-dbt-bnd;Bond"/>
		<rdfs:subClassOf rdf:resource="&fibo-sec-dbt-bnd;GovernmentIssuedDebtSecurity"/>
		<rdfs:label>government bond</rdfs:label>
		<skos:definition>debt security issued by a government to support government spending</skos:definition>
		<fibo-fnd-utl-av:explanatoryNote>Government bonds can pay periodic interest payments and are considered low-risk investments since the issuing government backs them.</fibo-fnd-utl-av:explanatoryNote>
		<fibo-fnd-utl-av:synonym>government-issued bond</fibo-fnd-utl-av:synonym>
	</owl:Class>
	
	<owl:Class rdf:about="&fibo-sec-dbt-bnd;GovernmentIssuedDebtSecurity">
		<rdfs:subClassOf rdf:resource="&fibo-sec-dbt-dbti;TradableDebtInstrument"/>
		<rdfs:subClassOf>
			<owl:Restriction>
				<owl:onProperty rdf:resource="&fibo-fnd-rel-rel;isIssuedBy"/>
				<owl:someValuesFrom>
					<owl:Restriction>
						<owl:onProperty rdf:resource="&fibo-fnd-pty-rl;isPlayedBy"/>
						<owl:someValuesFrom rdf:resource="&fibo-be-ge-ge;Polity"/>
					</owl:Restriction>
				</owl:someValuesFrom>
			</owl:Restriction>
		</rdfs:subClassOf>
		<rdfs:label>government issued debt security</rdfs:label>
		<skos:definition>a debt security issued by some government on behalf of some polity, including sovereign and municipal debt</skos:definition>
	</owl:Class>
	
	<owl:Class rdf:about="&fibo-sec-dbt-bnd;GreenBond">
		<rdfs:subClassOf rdf:resource="&fibo-sec-dbt-bnd;Bond"/>
		<rdfs:label>green bond</rdfs:label>
		<skos:definition>tax-exempt bond issued by federally qualified organizations or by municipalities for the development of brownfield sites</skos:definition>
		<fibo-fnd-utl-av:explanatoryNote>Brownfield sites are areas of land that are underutilized, have abandoned buildings or are underdeveloped, often containing low levels of industrial pollution.</fibo-fnd-utl-av:explanatoryNote>
	</owl:Class>
	
	<owl:Class rdf:about="&fibo-sec-dbt-bnd;HoldersOptionCall">
		<rdfs:subClassOf rdf:resource="&fibo-sec-dbt-bnd;PartialCallAllocation"/>
		<rdfs:label>holders option call</rdfs:label>
	</owl:Class>
	
	<owl:Class rdf:about="&fibo-sec-dbt-bnd;ImplicitFullFaithAndCreditBond">
		<rdfs:subClassOf rdf:resource="&fibo-sec-dbt-bnd;FullFaithAndCreditBond"/>
		<rdfs:label>implicit full faith and credit bond</rdfs:label>
		<skos:definition></skos:definition>
	</owl:Class>
	
	<owl:Class rdf:about="&fibo-sec-dbt-bnd;IndexAmortizingBond">
		<rdfs:subClassOf rdf:resource="&fibo-sec-dbt-bnd;AmortizingBond"/>
		<rdfs:subClassOf rdf:resource="&fibo-sec-dbt-bnd;IndexBasedCouponBond"/>
		<rdfs:subClassOf>
			<owl:Restriction>
				<owl:onProperty rdf:resource="&fibo-sec-dbt-dbti;hasRepaymentTerms"/>
				<owl:someValuesFrom rdf:resource="&fibo-sec-dbt-bnd;IndexLinkedPrincipalDeterminationTerms"/>
			</owl:Restriction>
		</rdfs:subClassOf>
		<rdfs:label>index amortizing bond</rdfs:label>
		<skos:definition></skos:definition>
	</owl:Class>
	
	<owl:Class rdf:about="&fibo-sec-dbt-bnd;IndexBasedCouponBond">
		<rdfs:subClassOf rdf:resource="&fibo-sec-dbt-bnd;VariableCouponBond"/>
		<rdfs:subClassOf>
			<owl:Restriction>
				<owl:onProperty rdf:resource="&fibo-fbc-dae-dbt;hasInterestRate"/>
				<owl:someValuesFrom rdf:resource="&fibo-sec-dbt-bnd;IndexLinkedCoupon"/>
			</owl:Restriction>
		</rdfs:subClassOf>
		<rdfs:subClassOf>
			<owl:Restriction>
				<owl:onProperty rdf:resource="&fibo-sec-dbt-dbti;hasInterestPaymentTerms"/>
				<owl:someValuesFrom rdf:resource="&fibo-sec-dbt-bnd;IndexLinkedCouponTerms"/>
			</owl:Restriction>
		</rdfs:subClassOf>
		<rdfs:label>index-based coupon bond</rdfs:label>
		<skos:definition>variable coupon bond with payments that fluctuate according to an &quot;index&quot; other than an interest rate, such as an economic indicator</skos:definition>
		<skos:editorialNote>Might also be referred to as Index Linked, but more commonly the term Index Linked refers to principal. So this term has a made up name for this kind of bond, following OTPP review in which we dealt with the distinction between index linked interest and index linked principal amounts. .</skos:editorialNote>
	</owl:Class>
	
	<owl:Class rdf:about="&fibo-sec-dbt-bnd;IndexLinkedCoupon">
		<rdfs:subClassOf rdf:resource="&fibo-sec-dbt-bnd;BondVariableCoupon"/>
		<rdfs:label>index linked coupon</rdfs:label>
		<owl:disjointWith rdf:resource="&fibo-sec-dbt-bnd;InflationBondVariableCoupon"/>
		<owl:disjointWith rdf:resource="&fibo-sec-dbt-bnd;WACBondCoupon"/>
	</owl:Class>
	
	<owl:Class rdf:about="&fibo-sec-dbt-bnd;IndexLinkedCouponTerms">
		<rdfs:subClassOf rdf:resource="&fibo-sec-dbt-bnd;VariableCouponTerms"/>
		<rdfs:subClassOf>
			<owl:Restriction>
				<owl:onProperty rdf:resource="&fibo-fbc-dae-dbt;isBasedOn"/>
				<owl:someValuesFrom>
					<owl:Class>
						<owl:unionOf rdf:parseType="Collection">
							<rdf:Description rdf:about="&fibo-ind-ei-ei;EconomicIndicator">
							</rdf:Description>
							<rdf:Description rdf:about="&fibo-ind-ind-ind;MarketRate">
							</rdf:Description>
						</owl:unionOf>
					</owl:Class>
				</owl:someValuesFrom>
			</owl:Restriction>
		</rdfs:subClassOf>
		<rdfs:label>index-linked coupon terms</rdfs:label>
	</owl:Class>
	
	<owl:Class rdf:about="&fibo-sec-dbt-bnd;IndexLinkedPrincipalDeterminationTerms">
		<rdfs:subClassOf rdf:resource="&fibo-sec-dbt-dbti;TradableDebtInstrumentRedemptionProvision"/>
		<rdfs:subClassOf>
			<owl:Restriction>
				<owl:onProperty rdf:resource="&fibo-fnd-utl-alx;hasExpression"/>
				<owl:someValuesFrom rdf:resource="&fibo-sec-dbt-bnd;PrincipalPaymentCalculation"/>
			</owl:Restriction>
		</rdfs:subClassOf>
		<rdfs:subClassOf>
			<owl:Restriction>
				<owl:onProperty rdf:resource="&fibo-sec-dbt-bnd;specifiesIndexParameter"/>
				<owl:someValuesFrom>
					<owl:Class>
						<owl:unionOf rdf:parseType="Collection">
							<rdf:Description rdf:about="&fibo-ind-ei-ei;EconomicIndicator">
							</rdf:Description>
							<rdf:Description rdf:about="&fibo-ind-ind-ind;MarketRate">
							</rdf:Description>
						</owl:unionOf>
					</owl:Class>
				</owl:someValuesFrom>
			</owl:Restriction>
		</rdfs:subClassOf>
		<rdfs:label>index-linked principal determination terms</rdfs:label>
		<skos:definition>terms for payment of the principal that tie the principal amounts to some underlying index or interest rate</skos:definition>
		<skos:editorialNote>Terms are linked to the calculation of the factor - see definition for Inflation Bond. This has been renamed from Principal Repayment Terms to Principal Determination Terms, since further review indicates a term whereby the principal amount itself varies, and this is borne out by the notes made at the original review, where this was mislabeled.</skos:editorialNote>
	</owl:Class>
	
	<owl:Class rdf:about="&fibo-sec-dbt-bnd;IndexLinkedSecurity">
		<rdfs:subClassOf rdf:resource="&fibo-sec-dbt-bnd;VariablePrincipalBond"/>
		<rdfs:subClassOf>
			<owl:Restriction>
				<owl:onProperty rdf:resource="&fibo-sec-dbt-bnd;isBasedOn"/>
				<owl:someValuesFrom>
					<owl:Class>
						<owl:unionOf rdf:parseType="Collection">
							<rdf:Description rdf:about="&fibo-ind-ei-ei;EconomicIndicator">
							</rdf:Description>
							<rdf:Description rdf:about="&fibo-ind-ind-ind;MarketRate">
							</rdf:Description>
						</owl:unionOf>
					</owl:Class>
				</owl:someValuesFrom>
			</owl:Restriction>
		</rdfs:subClassOf>
		<rdfs:label>index linked security</rdfs:label>
		<skos:definition>bond in which payment of income on the principal is related to a specific index, such as the Consumer Price Index</skos:definition>
		<fibo-fnd-utl-av:explanatoryNote>This feature provides protection to investors by shielding them from changes in the underlying index. The bond&apos;s cash flows are adjusted to ensure that the holder of the bond receives a known real rate of return. Notes 04 May: There may also be a kind of security where the coupon payments fluctuate according to an &quot;Index&quot; in the sense of non Interest rate e.g. inflation rate, GDP. But more commonly the term Index Linked refers to principal.</fibo-fnd-utl-av:explanatoryNote>
	</owl:Class>
	
	<owl:Class rdf:about="&fibo-sec-dbt-bnd;InflationBond">
		<rdfs:subClassOf rdf:resource="&fibo-sec-dbt-bnd;IndexLinkedSecurity"/>
		<rdfs:subClassOf>
			<owl:Restriction>
				<owl:onProperty rdf:resource="&fibo-sec-dbt-dbti;hasRepaymentTerms"/>
				<owl:onClass rdf:resource="&fibo-sec-dbt-bnd;IndexLinkedPrincipalDeterminationTerms"/>
				<owl:maxQualifiedCardinality rdf:datatype="&xsd;nonNegativeInteger">1</owl:maxQualifiedCardinality>
			</owl:Restriction>
		</rdfs:subClassOf>
		<rdfs:subClassOf>
			<owl:Restriction>
				<owl:onProperty rdf:resource="&fibo-sec-dbt-dbti;hasInterestPaymentTerms"/>
				<owl:someValuesFrom rdf:resource="&fibo-sec-dbt-bnd;InflationBondInterestPaymentTerms"/>
			</owl:Restriction>
		</rdfs:subClassOf>
		<rdfs:subClassOf>
			<owl:Restriction>
				<owl:onProperty rdf:resource="&fibo-sec-dbt-dbti;hasInterestPaymentTerms"/>
				<owl:someValuesFrom rdf:resource="&fibo-sec-dbt-bnd;InflationBondVariableCouponTerms"/>
			</owl:Restriction>
		</rdfs:subClassOf>
		<rdfs:subClassOf>
			<owl:Restriction>
				<owl:onProperty rdf:resource="&fibo-sec-dbt-dbti;hasRepaymentTerms"/>
				<owl:someValuesFrom rdf:resource="&fibo-sec-dbt-bnd;InflationBondPrincipalRepaymentTerms"/>
			</owl:Restriction>
		</rdfs:subClassOf>
		<rdfs:label>inflation bond</rdfs:label>
		<skos:definition>bond whose principal amount is linked to an inflation rate index</skos:definition>
		<fibo-fnd-utl-av:explanatoryNote>The inflation rate is used to define the factor or multiplier for the bond, that is the factor that you multiply the bond by. How this works is that you take the inflation rate when the security was issued, and the inflation rate at the present. The difference between these becomes the Factor, e.g. 100% -&amp;gt; 101% gives 1% so for example for a $1000 issue - calculate the principal on which the interest is paid AND the principal from the point of view of how the principal is repaid. Some inflation bonds only do this on interest, some only on interest, but most apply it to the principal and interest. Coupon interest calculated based on the adjusted amount of the bond. so a fixed coupon rate is multiplied by e.g. 1010 in the example above. Variations e.g. Italy - daily published factor published for that bond, whereas other calculate based on underlying index. Typically a CPI or a statistical number generated by the govt. typically a lagging three month index. See UK bonds on this. US and Japanese ones - look at inflation rate 3 months prior. Unlike an Amortizing Security this principal value of the bond is increasing, whereas for and Amortizing, the principal is decreasing. In Canada, these are also referred to as &quot;real return bonds&quot;. 
Further Notes:Additional review with OTPP May 05 2010 indicates that this is part of a classification of bonds where the principal amount itself varies according to some index, a point which was not understood at the original review session. Terms and labels revised to fit this picture.</fibo-fnd-utl-av:explanatoryNote>
	</owl:Class>
	
	<owl:Class rdf:about="&fibo-sec-dbt-bnd;InflationBondInterestPaymentTerms">
		<rdfs:subClassOf rdf:resource="&fibo-sec-dbt-bnd;CouponPaymentTerms"/>
		<rdfs:label>inflation bond interest payment terms</rdfs:label>
		<skos:definition>terms for the payment of interest on an inflation bond</skos:definition>
		<fibo-fnd-utl-av:explanatoryNote>These may for example specify that the interest payments are by way of coupone calculated with reference to the inflation rate that is referenced for that bond, or they may not (for example they may specify a fixed coupon amount). Therefore these terms may specify any potential interest payment arrangement used on bonds.</fibo-fnd-utl-av:explanatoryNote>
	</owl:Class>
	
	<owl:Class rdf:about="&fibo-sec-dbt-bnd;InflationBondPrincipalRepaymentTerms">
		<rdfs:subClassOf rdf:resource="&fibo-sec-dbt-bnd;IndexLinkedPrincipalDeterminationTerms"/>
		<rdfs:subClassOf>
			<owl:Restriction>
				<owl:onProperty rdf:resource="&fibo-fnd-utl-alx;hasExpression"/>
				<owl:someValuesFrom rdf:resource="&fibo-sec-dbt-bnd;InflationFactorExpression"/>
			</owl:Restriction>
		</rdfs:subClassOf>
		<rdfs:label>inflation bond principal repayment terms</rdfs:label>
		<skos:definition>terms specifying how the principal amount on an inflation bond is to be paid down</skos:definition>
		<fibo-fnd-utl-av:explanatoryNote>Further notes: This is typically but not necessarily with reference to the Inflation rate that is referred to for this bond. Further model action: identify and model terms for the case where the bond principal repayments are not pegged to an inflation rate.</fibo-fnd-utl-av:explanatoryNote>
	</owl:Class>
	
	<owl:Class rdf:about="&fibo-sec-dbt-bnd;InflationBondVariableCoupon">
		<rdfs:subClassOf rdf:resource="&fibo-sec-dbt-bnd;BondVariableCoupon"/>
		<rdfs:label>inflation bond variable coupon</rdfs:label>
		<owl:disjointWith rdf:resource="&fibo-sec-dbt-bnd;WACBondCoupon"/>
	</owl:Class>
	
	<owl:Class rdf:about="&fibo-sec-dbt-bnd;InflationBondVariableCouponTerms">
		<rdfs:subClassOf rdf:resource="&fibo-sec-dbt-bnd;VariableCouponTerms"/>
		<rdfs:subClassOf>
			<owl:Restriction>
				<owl:onProperty rdf:resource="&fibo-fbc-dae-dbt;hasInterestRate"/>
				<owl:onClass rdf:resource="&fibo-sec-dbt-bnd;InflationBondVariableCoupon"/>
				<owl:maxQualifiedCardinality rdf:datatype="&xsd;nonNegativeInteger">1</owl:maxQualifiedCardinality>
			</owl:Restriction>
		</rdfs:subClassOf>
		<rdfs:subClassOf>
			<owl:Restriction>
				<owl:onProperty rdf:resource="&fibo-fnd-utl-alx;hasExpression"/>
				<owl:someValuesFrom rdf:resource="&fibo-sec-dbt-bnd;InflationFactorExpression"/>
			</owl:Restriction>
		</rdfs:subClassOf>
		<rdfs:label>inflation bond variable coupon terms</rdfs:label>
	</owl:Class>
	
	<owl:Class rdf:about="&fibo-sec-dbt-bnd;InflationFactorExpression">
		<rdfs:subClassOf rdf:resource="&fibo-fnd-utl-alx;Expression"/>
		<rdfs:subClassOf>
			<owl:Restriction>
				<owl:onProperty rdf:resource="&fibo-fnd-utl-alx;hasArgument"/>
				<owl:someValuesFrom rdf:resource="&fibo-ind-ei-ei;InflationRate"/>
			</owl:Restriction>
		</rdfs:subClassOf>
		<rdfs:label>inflation factor expression</rdfs:label>
		<skos:definition>the expression used to calculate the outstanding principal of the bond due to changes in the inflation rate</skos:definition>
	</owl:Class>
	
	<owl:Class rdf:about="&fibo-sec-dbt-bnd;IssuersOptionCall">
		<rdfs:subClassOf rdf:resource="&fibo-sec-dbt-bnd;PartialCallAllocation"/>
		<rdfs:label>issuers option call</rdfs:label>
	</owl:Class>
	
	<owl:Class rdf:about="&fibo-sec-dbt-bnd;LastRegularCouponDate">
		<rdfs:subClassOf rdf:resource="&fibo-fnd-dt-fd;ExplicitDate"/>
		<rdfs:label>last regular coupon date</rdfs:label>
		<skos:definition>scheduled date of the last regular coupon payment, that is the last of the payments that are made according to a regular repeating series of coupon periods, before any non-standard (long or short) final coupon period in the schedule</skos:definition>
	</owl:Class>
	
	<owl:Class rdf:about="&fibo-sec-dbt-bnd;LimitedTaxGeneralObligationBond">
		<rdfs:subClassOf rdf:resource="&fibo-sec-dbt-bnd;GeneralObligationMunicipalBond"/>
		<rdfs:label>limited tax general obligation bond</rdfs:label>
		<skos:definition>general obligation municipal bond that includes a commitment by the issuer to raise property taxes if necessary to meet existing debt service obligations</skos:definition>
		<fibo-fnd-utl-av:explanatoryNote>However, this increase is bounded by a statutory limit. With limited-tax general obligation pledges, governments can still use a part of already-levied property taxes, use another stream of income, or raise property taxes to an amount equating to existing debt service payments to answer its debt obligations.</fibo-fnd-utl-av:explanatoryNote>
	</owl:Class>
	
	<owl:Class rdf:about="&fibo-sec-dbt-bnd;ListedBond">
		<rdfs:subClassOf rdf:resource="&fibo-sec-dbt-bnd;Bond"/>
		<rdfs:subClassOf rdf:resource="&fibo-sec-sec-lst;ExchangeTradedSecurity"/>
		<rdfs:subClassOf>
			<owl:Restriction>
				<owl:onProperty rdf:resource="&fibo-sec-sec-lst;isListedVia"/>
				<owl:someValuesFrom rdf:resource="&fibo-sec-dbt-bnd;BondListing"/>
			</owl:Restriction>
		</rdfs:subClassOf>
		<rdfs:label>listed bond</rdfs:label>
		<owl:disjointWith rdf:resource="&fibo-sec-dbt-bnd;UnlistedBond"/>
		<skos:definition>a bond that may be traded on one or more exchanges</skos:definition>
		<fibo-fnd-utl-av:explanatoryNote>In principle this may be any type of bond other than an unlisted bond. Most exchange traded bonds are corporate bonds (but most corporate bonds are not exchange traded bonds). This is a common but not a necessary fact.</fibo-fnd-utl-av:explanatoryNote>
	</owl:Class>
	
	<owl:Class rdf:about="&fibo-sec-dbt-bnd;LotteryCall">
		<rdfs:subClassOf rdf:resource="&fibo-sec-dbt-bnd;PartialCallAllocation"/>
		<rdfs:label>lottery call</rdfs:label>
	</owl:Class>
	
	<owl:Class rdf:about="&fibo-sec-dbt-bnd;MakeWholeCall">
		<rdfs:subClassOf rdf:resource="&fibo-sec-dbt-bnd;EntireCall"/>
		<rdfs:label>make whole call</rdfs:label>
	</owl:Class>
	
	<owl:Class rdf:about="&fibo-sec-dbt-bnd;MandatorySinkingFundTerms">
		<rdfs:subClassOf rdf:resource="&fibo-sec-dbt-bnd;BondAmortizationPaymentTerms"/>
		<rdfs:subClassOf>
			<owl:Restriction>
				<owl:onProperty rdf:resource="&fibo-fnd-dt-fd;hasSchedule"/>
				<owl:someValuesFrom rdf:resource="&fibo-sec-dbt-dbti;CallSchedule"/>
			</owl:Restriction>
		</rdfs:subClassOf>
		<rdfs:label>mandatory sinking fund description</rdfs:label>
		<skos:definition>terms relating to a mandatory sinking fund call of the issue</skos:definition>
	</owl:Class>
	
	<owl:Class rdf:about="&fibo-sec-dbt-bnd;MediumTermNote">
		<rdfs:subClassOf rdf:resource="&fibo-sec-dbt-bnd;Bond"/>
		<rdfs:label>medium term note</rdfs:label>
		<skos:definition>negotiable debt instrument offered under a program agreement through one or more dealers on request of the issuer</skos:definition>
		<fibo-fnd-utl-av:explanatoryNote>MTNs have a maturity typically of 1 to 10 years. This may vary in different jurisductions. Bonds issued with a long maturity are not redefined as MTNs when their maturity reduces. MTN typically has a long last coupon payment. Some things are different from regular bonds, e.g.: You can register one with different maturities, issued in different groups (cf tranches). See also shelf registration (issuing bond before you file the paperwork with e.g. SEC - not the same). In this case it is registered but not issued all at one time. Flexible. Difference with bond issuance is that you have indenture that says what the maturity is, so every different maturity is a different bond.</fibo-fnd-utl-av:explanatoryNote>
		<fibo-fnd-utl-av:explanatoryNote>The Program defines the terms and conditions of the notes. An MTN issue is defined by the fact that the registration doesn&apos;t have a pre-defined maturity.</fibo-fnd-utl-av:explanatoryNote>
	</owl:Class>
	
	<owl:Class rdf:about="&fibo-sec-dbt-bnd;MunicipalBond">
		<rdfs:subClassOf rdf:resource="&fibo-sec-dbt-bnd;GovernmentBond"/>
		<rdfs:subClassOf rdf:resource="&fibo-sec-dbt-bnd;MunicipalSecurity"/>
		<rdfs:label>municipal bond</rdfs:label>
		<skos:definition>government bond that may be issued by states, cities, counties, special tax districts or special agencies or authorities of state or local governments</skos:definition>
	</owl:Class>
	
	<owl:Class rdf:about="&fibo-sec-dbt-bnd;MunicipalDebtFundsUsage">
		<rdfs:subClassOf rdf:resource="&fibo-be-le-lp;PublicPurpose"/>
		<rdfs:label>municipal debt funds usage</rdfs:label>
		<skos:definition>official statement identifying the application of funds in connection with a new issue of municipal securities</skos:definition>
	</owl:Class>
	
	<owl:Class rdf:about="&fibo-sec-dbt-bnd;MunicipalDebtObligor">
		<rdfs:subClassOf rdf:resource="&fibo-fnd-agr-agr;Obligor"/>
		<rdfs:subClassOf rdf:resource="&fibo-fnd-agr-ctr;ContractThirdParty"/>
		<rdfs:label>municipal debt obligor</rdfs:label>
		<skos:definition>party having a financial obligation or arrangement to make the payment of all or part of debt service on municipal securities</skos:definition>
		<fibo-fnd-utl-av:explanatoryNote>The obligor is often the issuer but may be a conduit borrower of municipal securities proceeds.</fibo-fnd-utl-av:explanatoryNote>
	</owl:Class>
	
	<owl:Class rdf:about="&fibo-sec-dbt-bnd;MunicipalDebtRemarketingAgent">
		<rdfs:subClassOf rdf:resource="&fibo-fbc-pas-fpas;Dealer"/>
		<rdfs:subClassOf rdf:resource="&fibo-fnd-agr-ctr;ContractThirdParty"/>
		<rdfs:label>municipal debt remarketing agent</rdfs:label>
		<skos:definition>municipal securities dealer responsible for reselling to investors securities (such as variable rate demand obligations and other tender option bonds) that have been tendered for purchase by their owner</skos:definition>
		<fibo-fnd-utl-av:explanatoryNote>The remarketing agent also typically is responsible for resetting the interest rate for a variable rate issue and may act as tender agent.</fibo-fnd-utl-av:explanatoryNote>
	</owl:Class>
	
	<owl:Class rdf:about="&fibo-sec-dbt-bnd;MunicipalNote">
		<rdfs:subClassOf rdf:resource="&fibo-sec-dbt-bnd;MunicipalSecurity"/>
		<rdfs:label>municipal note</rdfs:label>
		<skos:definition>short-term obligation to repay a specified principal amount on a certain date, together with interest at a stated rate, usually payable from a defined source of anticipated revenues</skos:definition>
		<fibo-fnd-utl-av:explanatoryNote>Notes usually mature in one year or less, although notes of longer maturities are also issued.</fibo-fnd-utl-av:explanatoryNote>
	</owl:Class>
	
	<owl:Class rdf:about="&fibo-sec-dbt-bnd;MunicipalSecurity">
		<rdfs:subClassOf rdf:resource="&fibo-sec-dbt-bnd;GovernmentIssuedDebtSecurity"/>
		<rdfs:subClassOf>
			<owl:Restriction>
				<owl:onProperty rdf:resource="&fibo-be-le-lp;hasObjective"/>
				<owl:someValuesFrom rdf:resource="&fibo-sec-dbt-bnd;MunicipalDebtFundsUsage"/>
			</owl:Restriction>
		</rdfs:subClassOf>
		<rdfs:subClassOf>
			<owl:Restriction>
				<owl:onProperty rdf:resource="&fibo-fnd-rel-rel;isIssuedBy"/>
				<owl:someValuesFrom>
					<owl:Restriction>
						<owl:onProperty rdf:resource="&fibo-fnd-pty-rl;isPlayedBy"/>
						<owl:someValuesFrom rdf:resource="&fibo-be-ge-ge;MunicipalEntity"/>
					</owl:Restriction>
				</owl:someValuesFrom>
			</owl:Restriction>
		</rdfs:subClassOf>
		<rdfs:label>municipal security</rdfs:label>
		<owl:disjointWith rdf:resource="&fibo-sec-dbt-bnd;SovereignDebtInstrument"/>
		<skos:definition>a bond, note, warrant, certificate of participation or other obligation issued by a state or local government or their agencies or authorities (such as cities, towns, villages, counties or special districts or authorities)</skos:definition>
		<fibo-fnd-utl-av:explanatoryNote>A prime feature of most municipal securities is that interest or other investment earnings on them are generally excluded from gross income of the bondholder for federal income tax purposes. Some municipal securities are subject to federal income tax, although the issuers or bondholders may receive other federal tax advantages for certain types of taxable municipal securities. Some examples include Build America Bonds, municipal fund securities and direct pay subsidy bonds.</fibo-fnd-utl-av:explanatoryNote>
	</owl:Class>
	
	<owl:Class rdf:about="&fibo-sec-dbt-bnd;MunicipalTrustee">
		<rdfs:subClassOf rdf:resource="&fibo-fnd-agr-ctr;ContractThirdParty"/>
		<rdfs:label>municipal trustee</rdfs:label>
		<skos:definition>financial institution with trust powers, designated by the issuer or borrower, that acts, pursuant to a bond contract, in a fiduciary capacity for the benefit of the bondholders in enforcing the terms of the bond contract</skos:definition>
		<fibo-fnd-utl-av:explanatoryNote>In many cases, the trustee also acts as custodian, paying agent, registrar and/or transfer agent for the bonds.</fibo-fnd-utl-av:explanatoryNote>
	</owl:Class>
	
	<owl:Class rdf:about="&fibo-sec-dbt-bnd;PartialCall">
		<rdfs:subClassOf rdf:resource="&fibo-sec-dbt-dbti;CallEvent"/>
		<rdfs:subClassOf>
			<owl:Restriction>
				<owl:onProperty rdf:resource="&fibo-sec-dbt-bnd;hasCallRedemptionType"/>
				<owl:someValuesFrom rdf:resource="&fibo-sec-dbt-bnd;PartialCallAllocation"/>
			</owl:Restriction>
		</rdfs:subClassOf>
		<rdfs:label>partial call</rdfs:label>
		<skos:definition>a call of part of the issue</skos:definition>
	</owl:Class>
	
	<owl:Class rdf:about="&fibo-sec-dbt-bnd;PartialCallAllocation">
		<rdfs:subClassOf rdf:resource="&fibo-fnd-dt-bd;Convention"/>
		<rdfs:label>partial call allocation</rdfs:label>
	</owl:Class>
	
	<owl:Class rdf:about="&fibo-sec-dbt-bnd;PartialCallFeature">
		<rdfs:subClassOf rdf:resource="&fibo-sec-dbt-dbti;CallFeature"/>
		<rdfs:label>partial call feature</rdfs:label>
		<skos:definition>call feature whereby the issuer can recall part of the issue on scheduled dates but there is no specific amount defined for those dates</skos:definition>
	</owl:Class>
	
	<owl:Class rdf:about="&fibo-sec-dbt-bnd;PercentageCAV">
		<rdfs:subClassOf rdf:resource="&fibo-sec-dbt-bnd;RateBasisType"/>
		<rdfs:label xml:lang="en">percentage c a v</rdfs:label>
		<skos:definition xml:lang="en">Percentage specified as percent of CAV (Cumulative Average Value)</skos:definition>
	</owl:Class>
	
	<owl:Class rdf:about="&fibo-sec-dbt-bnd;PercentagePar">
		<rdfs:subClassOf rdf:resource="&fibo-sec-dbt-bnd;RateBasisType"/>
		<rdfs:label xml:lang="en">percentage par</rdfs:label>
		<skos:definition xml:lang="en">Figure specified as a percentage of Par Value</skos:definition>
	</owl:Class>
	
	<owl:Class rdf:about="&fibo-sec-dbt-bnd;PerpetualBond">
		<rdfs:subClassOf rdf:resource="&fibo-sec-dbt-bnd;Bond"/>
		<rdfs:label xml:lang="en">perpetual bond</rdfs:label>
		<skos:definition xml:lang="en">a bond that has no maturity date, i.e., one that pays interest in perpetuity</skos:definition>
		<fibo-fnd-utl-av:explanatoryNote xml:lang="en">Perpetual bonds function much like dividend-paying stocks or certain preferred securities. Just as the owner of the stock receives a dividend payment as long as the stock is held, the perpetual bond owner receives an interest payment as long as the bond is held.</fibo-fnd-utl-av:explanatoryNote>
	</owl:Class>
	
	<owl:Class rdf:about="&fibo-sec-dbt-bnd;PerpetualFloatingRateNote">
		<rdfs:subClassOf rdf:resource="&fibo-sec-dbt-bnd;FloatingRateNote"/>
		<rdfs:label xml:lang="en">perpetual floating rate note</rdfs:label>
		<skos:definition xml:lang="en">A Floating Rate Note in which ... information to follow.</skos:definition>
		<skos:editorialNote xml:lang="en">Added as part of Corporate Actions and Events reviews. THere is an action (Remarketin gAgreement) which refers explicitly to Perpetual Floating Rate Notes. These had not previously been identified as a specific class of securities. Actions: Identify what terms (hopefully existing ones) come together to classify something as a perpetual FRN (presumably, it is one where there is no Maturity date, i.e. a Perpetual Bond?)</skos:editorialNote>
	</owl:Class>
	
	<owl:Class rdf:about="&fibo-sec-dbt-bnd;PrincipalPaymentCalculation">
		<rdfs:subClassOf rdf:resource="&fibo-fnd-utl-alx;Expression"/>
		<rdfs:subClassOf>
			<owl:Restriction>
				<owl:onProperty rdf:resource="&fibo-fnd-utl-alx;hasArgument"/>
				<owl:someValuesFrom rdf:resource="&fibo-fbc-dae-dbt;Principal"/>
			</owl:Restriction>
		</rdfs:subClassOf>
		<rdfs:label xml:lang="en">principal payment calculation</rdfs:label>
		<skos:definition xml:lang="en">a formula for calculation of principal payments for certain kinds of bonds</skos:definition>
	</owl:Class>
	
	<owl:Class rdf:about="&fibo-sec-dbt-bnd;ProRataCall">
		<rdfs:subClassOf rdf:resource="&fibo-sec-dbt-bnd;PartialCallAllocation"/>
		<rdfs:label xml:lang="en">pro rata call</rdfs:label>
	</owl:Class>
	
	<owl:Class rdf:about="&fibo-sec-dbt-bnd;RateBasisType">
		<rdfs:subClassOf rdf:resource="&fibo-fnd-dt-bd;Convention"/>
		<rdfs:label xml:lang="en">rate basis type</rdfs:label>
		<skos:definition xml:lang="en">The type of basis for a percentage quoted figure, as used in specifying Bond Call percentage amounts. REVIEW: Does this same meaningful term have wider applicability?</skos:definition>
	</owl:Class>
	
	<owl:Class rdf:about="&fibo-sec-dbt-bnd;RedemptionPayment">
		<rdfs:subClassOf rdf:resource="&fibo-fnd-pas-psch;PaymentEvent"/>
		<rdfs:subClassOf rdf:resource="&fibo-sec-dbt-dbti;RedemptionEvent"/>
		<rdfs:label xml:lang="en">redemption payment</rdfs:label>
	</owl:Class>
	
	<owl:Class rdf:about="&fibo-sec-dbt-bnd;RedemptionSchedule">
		<rdfs:subClassOf rdf:resource="&fibo-fnd-dt-fd;Schedule"/>
		<rdfs:subClassOf>
			<owl:Restriction>
				<owl:onProperty rdf:resource="&fibo-fnd-rel-rel;comprises"/>
				<owl:someValuesFrom rdf:resource="&fibo-sec-dbt-dbti;RedemptionEvent"/>
			</owl:Restriction>
		</rdfs:subClassOf>
		<rdfs:label xml:lang="en">redemption schedule</rdfs:label>
	</owl:Class>
	
	<owl:Class rdf:about="&fibo-sec-dbt-bnd;RegularCall">
		<rdfs:subClassOf rdf:resource="&fibo-sec-dbt-bnd;EntireCall"/>
		<rdfs:label xml:lang="en">regular call</rdfs:label>
	</owl:Class>
	
	<owl:Class rdf:about="&fibo-sec-dbt-bnd;RegularCouponSchedule">
		<rdfs:subClassOf rdf:resource="&fibo-fnd-dt-fd;RegularSchedule"/>
		<rdfs:subClassOf rdf:resource="&fibo-sec-dbt-bnd;CouponSchedule"/>
		<rdfs:label xml:lang="en">regular coupon schedule</rdfs:label>
		<skos:definition xml:lang="en">a schedule including an initial and/or final stub period and an interval of regular coupon payment dates</skos:definition>
	</owl:Class>
	
	<owl:Class rdf:about="&fibo-sec-dbt-bnd;RegulatoryCall">
		<rdfs:subClassOf rdf:resource="&fibo-sec-dbt-bnd;EntireCall"/>
		<rdfs:label xml:lang="en">regulatory call</rdfs:label>
	</owl:Class>
	
	<owl:Class rdf:about="&fibo-sec-dbt-bnd;RevenueBond">
		<rdfs:subClassOf rdf:resource="&fibo-sec-dbt-bnd;MunicipalBond"/>
		<rdfs:label xml:lang="en">revenue bond</rdfs:label>
		<skos:definition xml:lang="en">A revenue bond is a municipal bond supported by the revenue from a specific project, such as a toll bridge, highway or local stadium. Revenue bonds are municipal bonds that finance income-producing projects and are secured by a specified revenue source. Typically, revenue bonds can be issued by any government agency or fund that is managed in the manner of a business, such as entities having both operating revenues and expenses.</skos:definition>
	</owl:Class>
	
	<owl:Class rdf:about="&fibo-sec-dbt-bnd;SerialNumberCall">
		<rdfs:subClassOf rdf:resource="&fibo-sec-dbt-bnd;PartialCallAllocation"/>
		<rdfs:label xml:lang="en">serial number call</rdfs:label>
	</owl:Class>
	
	<owl:Class rdf:about="&fibo-sec-dbt-bnd;SingleCouponTerms">
		<rdfs:subClassOf rdf:resource="&fibo-sec-dbt-bnd;CouponPaymentTerms"/>
		<rdfs:label xml:lang="en">single coupon type</rdfs:label>
		<owl:disjointWith rdf:resource="&fibo-sec-dbt-bnd;SteppedCouponTerms"/>
		<skos:definition xml:lang="en">A set of coupon terms which remain the same through the life of the Bond. This is the default and is the case when there is not a Step Coupon or Conditional Coupon.</skos:definition>
	</owl:Class>
	
	<owl:Class rdf:about="&fibo-sec-dbt-bnd;SinkingFundAmortizationTerms">
		<rdfs:subClassOf>
			<owl:Restriction>
				<owl:onProperty rdf:resource="&fibo-fnd-dt-fd;hasSchedule"/>
				<owl:someValuesFrom rdf:resource="&fibo-sec-dbt-bnd;RedemptionSchedule"/>
			</owl:Restriction>
		</rdfs:subClassOf>
		<rdfs:label xml:lang="en">published sinking fund amortization terms description</rdfs:label>
		<skos:definition xml:lang="en">Terms for the paydown of principal in a sinking fund type of amortizing security.</skos:definition>
		<skos:editorialNote xml:lang="en">At present there is only a schedule, there should be other terms for what happens on the scheduled dates. Sinking fund may be bullet e.g. x% over year for y years. SF may be mandatory or contingent on some other economic event.</skos:editorialNote>
	</owl:Class>
	
	<owl:Class rdf:about="&fibo-sec-dbt-bnd;SovereignBond">
		<rdfs:subClassOf rdf:resource="&fibo-sec-dbt-bnd;FullFaithAndCreditBond"/>
		<rdfs:subClassOf rdf:resource="&fibo-sec-dbt-bnd;GovernmentBond"/>
		<rdfs:subClassOf rdf:resource="&fibo-sec-dbt-bnd;SovereignDebtInstrument"/>
		<rdfs:label xml:lang="en">sovereign bond</rdfs:label>
	</owl:Class>
	
	<owl:Class rdf:about="&fibo-sec-dbt-bnd;SovereignDebtInstrument">
		<rdfs:subClassOf rdf:resource="&fibo-sec-dbt-bnd;GovernmentIssuedDebtSecurity"/>
		<rdfs:subClassOf>
			<owl:Restriction>
				<owl:onProperty rdf:resource="&fibo-fnd-rel-rel;isIssuedBy"/>
				<owl:someValuesFrom>
					<owl:Restriction>
						<owl:onProperty rdf:resource="&fibo-fnd-pty-rl;isPlayedBy"/>
						<owl:someValuesFrom rdf:resource="&fibo-be-ge-ge;SovereignState"/>
					</owl:Restriction>
				</owl:someValuesFrom>
			</owl:Restriction>
		</rdfs:subClassOf>
		<rdfs:label xml:lang="en">sovereign debt instrument</rdfs:label>
	</owl:Class>
	
	<owl:Class rdf:about="&fibo-sec-dbt-bnd;SpecialAssessmentBond">
		<rdfs:subClassOf rdf:resource="&fibo-sec-dbt-bnd;MunicipalBond"/>
		<rdfs:label xml:lang="en">special assessment bond</rdfs:label>
		<skos:definition xml:lang="en">An obligation payable from revenues of a special assessment. A special assessment is a charge imposed against a property in a particular locality because that property receives a special benefit by virtue of some public improvement, separate and apart from the general benefit accruing to the public at large. Special assessments may be apportioned according to the value of the benefit received, rather than merely the cost of the improvement.</skos:definition>
	</owl:Class>
	
	<owl:Class rdf:about="&fibo-sec-dbt-bnd;SpecialCall">
		<rdfs:subClassOf rdf:resource="&fibo-sec-dbt-bnd;EntireCall"/>
		<rdfs:label xml:lang="en">special call</rdfs:label>
	</owl:Class>
	
	<owl:Class rdf:about="&fibo-sec-dbt-bnd;SpecialObligationBond">
		<rdfs:subClassOf rdf:resource="&fibo-sec-dbt-bnd;MunicipalBond"/>
		<rdfs:label xml:lang="en">special obligation bond</rdfs:label>
		<skos:definition xml:lang="en">A bond secured by a limited revenue source or promise to pay.</skos:definition>
	</owl:Class>
	
	<owl:Class rdf:about="&fibo-sec-dbt-bnd;SpecialTaxBond">
		<rdfs:subClassOf rdf:resource="&fibo-sec-dbt-bnd;MunicipalBond"/>
		<rdfs:label xml:lang="en">special tax bond</rdfs:label>
		<skos:definition xml:lang="en">A bond secured by revenues derived from one or more designated taxes other than ad valorem taxes. For example, bonds for a particular purpose might be supported by sales, cigarette, fuel or business license taxes.</skos:definition>
	</owl:Class>
	
	<owl:Class rdf:about="&fibo-sec-dbt-bnd;StepEvent">
		<rdfs:subClassOf rdf:resource="&fibo-sec-dbt-dbti;PrescriptiveEvent"/>
		<rdfs:subClassOf>
			<owl:Restriction>
				<owl:onProperty rdf:resource="&fibo-fnd-rel-rel;involves"/>
				<owl:someValuesFrom rdf:resource="&fibo-sec-dbt-bnd;FixedCouponTerms"/>
			</owl:Restriction>
		</rdfs:subClassOf>
		<rdfs:label>step event</rdfs:label>
		<skos:definition>an event whereby a set of fixed coupon terms comes into force as specified in a step schedule</skos:definition>
	</owl:Class>
	
	<owl:Class rdf:about="&fibo-sec-dbt-bnd;StepSchedule">
		<rdfs:subClassOf rdf:resource="&fibo-fnd-dt-fd;AdHocSchedule"/>
		<rdfs:subClassOf>
			<owl:Restriction>
				<owl:onProperty rdf:resource="&fibo-fnd-rel-rel;comprises"/>
				<owl:someValuesFrom rdf:resource="&fibo-sec-dbt-bnd;StepEvent"/>
			</owl:Restriction>
		</rdfs:subClassOf>
		<rdfs:label xml:lang="en">step schedule</rdfs:label>
	</owl:Class>
	
	<owl:Class rdf:about="&fibo-sec-dbt-bnd;StepUpBond">
		<rdfs:subClassOf rdf:resource="&fibo-sec-dbt-bnd;Bond"/>
		<rdfs:subClassOf>
			<owl:Restriction>
				<owl:onProperty rdf:resource="&fibo-sec-dbt-dbti;hasInterestPaymentTerms"/>
				<owl:someValuesFrom rdf:resource="&fibo-sec-dbt-bnd;SteppedCouponTerms"/>
			</owl:Restriction>
		</rdfs:subClassOf>
		<rdfs:label xml:lang="en">step up bond</rdfs:label>
		<skos:definition xml:lang="en">a bond with a coupon that increases (steps up), usually at regular intervals, while the bond is outstanding</skos:definition>
	</owl:Class>
	
	<owl:Class rdf:about="&fibo-sec-dbt-bnd;SteppedCouponTerms">
		<rdfs:subClassOf rdf:resource="&fibo-sec-dbt-bnd;CouponPaymentTerms"/>
		<rdfs:subClassOf>
			<owl:Restriction>
				<owl:onProperty rdf:resource="&fibo-fnd-dt-fd;hasSchedule"/>
				<owl:someValuesFrom rdf:resource="&fibo-sec-dbt-bnd;StepSchedule"/>
			</owl:Restriction>
		</rdfs:subClassOf>
		<rdfs:label xml:lang="en">stepped coupon type</rdfs:label>
	</owl:Class>
	
	<owl:Class rdf:about="&fibo-sec-dbt-bnd;StripBond">
		<rdfs:subClassOf rdf:resource="&fibo-sec-dbt-bnd;ZeroCouponBond"/>
		<rdfs:subClassOf rdf:resource="&fibo-sec-dbt-dbti;PrincipalOnlyStrip"/>
		<rdfs:subClassOf>
			<owl:Restriction>
				<owl:onProperty rdf:resource="&fibo-fbc-dae-dbt;isBasedOn"/>
				<owl:someValuesFrom rdf:resource="&fibo-sec-dbt-bnd;Bond"/>
			</owl:Restriction>
		</rdfs:subClassOf>
		<rdfs:label xml:lang="en">strip bond</rdfs:label>
		<skos:definition xml:lang="en">a bond created through the process of removing coupons from a bond and then selling the separate parts as a zero coupon bond and an interest paying coupon bond</skos:definition>
	</owl:Class>
	
	<owl:Class rdf:about="&fibo-sec-dbt-bnd;TaxAllocationBond">
		<rdfs:subClassOf rdf:resource="&fibo-sec-dbt-bnd;MunicipalBond"/>
		<rdfs:label xml:lang="en">tax allocation bond</rdfs:label>
		<skos:definition xml:lang="en">A bond payable from the incremental increase in tax revenues realized from any increase in property value and other economic activity, often designed to capture the economic benefit resulting from a bond financing. Tax increment bonds, also known as tax allocation bonds, often are used to finance the redevelopment of blighted areas.</skos:definition>
	</owl:Class>
	
	<owl:Class rdf:about="&fibo-sec-dbt-bnd;TreasuryBill">
		<rdfs:subClassOf rdf:resource="&fibo-sec-dbt-bnd;SovereignDebtInstrument"/>
		<rdfs:subClassOf rdf:resource="&fibo-sec-dbt-tstd;MoneyMarketInstrument"/>
		<rdfs:subClassOf>
			<owl:Restriction>
				<owl:onProperty rdf:resource="&fibo-sec-dbt-dbti;hasRelativePriceAtIssue"/>
				<owl:hasValue rdf:resource="&fibo-sec-dbt-dbti;AtADiscount"/>
			</owl:Restriction>
		</rdfs:subClassOf>
		<rdfs:subClassOf>
			<owl:Restriction>
				<owl:onProperty rdf:resource="&fibo-sec-dbt-dbti;hasRelativePriceAtMaturity"/>
				<owl:hasValue rdf:resource="&fibo-sec-dbt-dbti;ParValue"/>
			</owl:Restriction>
		</rdfs:subClassOf>
		<rdfs:subClassOf>
			<owl:Restriction>
				<owl:onProperty rdf:resource="&fibo-fbc-dae-dbt;hasInterestRate"/>
				<owl:someValuesFrom rdf:resource="&fibo-ind-ir-ir;ReferenceInterestRate"/>
			</owl:Restriction>
		</rdfs:subClassOf>
		<rdfs:label xml:lang="en">treasury bill</rdfs:label>
		<skos:definition xml:lang="en">a short-term debt obligation backed by the Treasury Department of the U.S. government with a maturity of less than one year, sold in denominations of $1,000 up to a maximum purchase of $5 million on noncompetitive bids</skos:definition>
		<fibo-fnd-utl-av:abbreviation xml:lang="en">T-bill</fibo-fnd-utl-av:abbreviation>
	</owl:Class>
	
	<owl:Class rdf:about="&fibo-sec-dbt-bnd;TrusteeCall">
		<rdfs:subClassOf rdf:resource="&fibo-sec-dbt-bnd;EntireCall"/>
		<rdfs:label xml:lang="en">trustee call</rdfs:label>
	</owl:Class>
	
	<owl:Class rdf:about="&fibo-sec-dbt-bnd;UnlimitedTaxGeneralObligationBond">
		<rdfs:subClassOf rdf:resource="&fibo-sec-dbt-bnd;GeneralObligationMunicipalBond"/>
		<rdfs:label xml:lang="en">unlimited tax general obligation bond</rdfs:label>
		<skos:definition xml:lang="en">An unlimited-tax general obligation pledge is similar to the limited-tax pledge. The only difference is that the local government is asked to increase property tax rates to necessary levels - up to a maximum of 100% - to cover delinquencies from taxpayers. Local residents must first agree to increase property taxes to necessary amounts required for the bonds.</skos:definition>
	</owl:Class>
	
	<owl:Class rdf:about="&fibo-sec-dbt-bnd;UnlistedBond">
		<rdfs:subClassOf rdf:resource="&fibo-sec-dbt-bnd;Bond"/>
		<rdfs:label xml:lang="en">unlisted bond</rdfs:label>
		<skos:definition xml:lang="en">A bond that is traded over the counter rather than via an exchange or other listing facility.</skos:definition>
		<fibo-fnd-utl-av:synonym xml:lang="en">OTC Bond</fibo-fnd-utl-av:synonym>
	</owl:Class>
	
	<owl:Class rdf:about="&fibo-sec-dbt-bnd;VariableCouponBond">
		<rdfs:subClassOf rdf:resource="&fibo-sec-dbt-bnd;Bond"/>
		<rdfs:subClassOf>
			<owl:Restriction>
				<owl:onProperty rdf:resource="&fibo-fbc-dae-dbt;hasInterestRate"/>
				<owl:someValuesFrom rdf:resource="&fibo-sec-dbt-bnd;BondVariableCoupon"/>
			</owl:Restriction>
		</rdfs:subClassOf>
		<rdfs:label>variable coupon bond</rdfs:label>
		<skos:definition>a bond that has a floating or variable interest rate, or coupon rate</skos:definition>
		<fibo-fnd-utl-av:explanatoryNote>The rate adjusts according to a predetermined formula outlined in the bond&apos;s prospectus or official statement.</fibo-fnd-utl-av:explanatoryNote>
	</owl:Class>
	
	<owl:Class rdf:about="&fibo-sec-dbt-bnd;VariableCouponTerms">
		<rdfs:subClassOf rdf:resource="&fibo-sec-dbt-bnd;CouponPaymentTerms"/>
		<rdfs:subClassOf>
			<owl:Restriction>
				<owl:onProperty rdf:resource="&fibo-fbc-dae-dbt;isBasedOn"/>
				<owl:someValuesFrom rdf:resource="&fibo-ind-ind-ind;MarketRate"/>
			</owl:Restriction>
		</rdfs:subClassOf>
		<rdfs:subClassOf>
			<owl:Restriction>
				<owl:onProperty rdf:resource="&fibo-fnd-utl-alx;hasExpression"/>
				<owl:someValuesFrom rdf:resource="&fibo-sec-dbt-bnd;VariableInterestCalculationFormula"/>
			</owl:Restriction>
		</rdfs:subClassOf>
		<rdfs:label xml:lang="en">bond variable coupon terms</rdfs:label>
	</owl:Class>
	
	<owl:Class rdf:about="&fibo-sec-dbt-bnd;VariableDebtPrincipal">
		<rdfs:subClassOf rdf:resource="&fibo-sec-dbt-dbti;PubliclyIssuedDebt"/>
		<rdfs:label xml:lang="en">variable debt principal</rdfs:label>
		<skos:definition xml:lang="en">An amount of issued debt principal which is defined in relation to some variable and so varies over time, as principal.</skos:definition>
		<fibo-fnd-utl-av:explanatoryNote xml:lang="en">Not the same as principal paydown. This is when the principal itself varies over time, usually as a result of being defined in relation to some index such as an inflation index. Forms the debt principal in instruments such as inflation bonds.</fibo-fnd-utl-av:explanatoryNote>
	</owl:Class>
	
	<owl:Class rdf:about="&fibo-sec-dbt-bnd;VariableInterestCalculationFormula">
		<rdfs:subClassOf rdf:resource="&fibo-sec-dbt-dbti;FullyIndexedInterestRate"/>
		<rdfs:label xml:lang="en">variable interest calculation formula</rdfs:label>
		<skos:definition xml:lang="en">Formula for the calculation of variable interest.</skos:definition>
		<skos:editorialNote xml:lang="en">This inherits all the facts about Interest Calculation Formula without alteration.</skos:editorialNote>
	</owl:Class>
	
	<owl:Class rdf:about="&fibo-sec-dbt-bnd;VariableInterestExpression">
		<rdfs:subClassOf rdf:resource="&fibo-fnd-utl-alx;Expression"/>
		<rdfs:subClassOf>
			<owl:Restriction>
				<owl:onProperty rdf:resource="&fibo-sec-dbt-bnd;cap"/>
				<owl:onClass rdf:resource="&fibo-fnd-utl-val;PercentageValue"/>
				<owl:maxQualifiedCardinality rdf:datatype="&xsd;nonNegativeInteger">1</owl:maxQualifiedCardinality>
			</owl:Restriction>
		</rdfs:subClassOf>
		<rdfs:subClassOf>
			<owl:Restriction>
				<owl:onProperty rdf:resource="&fibo-sec-dbt-bnd;floor"/>
				<owl:onClass rdf:resource="&fibo-fnd-utl-val;PercentageValue"/>
				<owl:maxQualifiedCardinality rdf:datatype="&xsd;nonNegativeInteger">1</owl:maxQualifiedCardinality>
			</owl:Restriction>
		</rdfs:subClassOf>
		<rdfs:subClassOf>
			<owl:Restriction>
				<owl:onProperty rdf:resource="&fibo-fnd-utl-alx;hasArgument"/>
				<owl:onClass rdf:resource="&fibo-sec-dbt-dbti;FullyIndexedInterestRate"/>
				<owl:qualifiedCardinality rdf:datatype="&xsd;nonNegativeInteger">1</owl:qualifiedCardinality>
			</owl:Restriction>
		</rdfs:subClassOf>
		<rdfs:label xml:lang="en">variable interest expression</rdfs:label>
		<skos:definition xml:lang="en">an expression used to determine a variable interest payment amount</skos:definition>
	</owl:Class>
	
	<owl:Class rdf:about="&fibo-sec-dbt-bnd;VariablePrincipalBond">
		<rdfs:subClassOf rdf:resource="&fibo-sec-dbt-bnd;Bond"/>
		<rdfs:subClassOf>
			<owl:Restriction>
				<owl:onProperty rdf:resource="&fibo-fnd-agr-ctr;definesTermsFor"/>
				<owl:someValuesFrom rdf:resource="&fibo-sec-dbt-bnd;VariableDebtPrincipal"/>
			</owl:Restriction>
		</rdfs:subClassOf>
		<rdfs:label xml:lang="en">variable principal bond</rdfs:label>
		<skos:definition xml:lang="en">A bond where the actual principal amount may vary, other than through paydown of the principal as amortization.</skos:definition>
		<fibo-fnd-utl-av:explanatoryNote xml:lang="en">This would typically be a bond where the principal is not a fixed amount but is varied according to some index, that is the actual amount of the debt itself varies, independently of whether the principal is amortized or not, and regardless of whether the coupon is fixed or variable (though a coupon of a fixed percentage would translate to a variable monetary amount).</fibo-fnd-utl-av:explanatoryNote>
	</owl:Class>
	
	<owl:Class rdf:about="&fibo-sec-dbt-bnd;WACBondCoupon">
		<rdfs:subClassOf rdf:resource="&fibo-sec-dbt-bnd;BondVariableCoupon"/>
		<rdfs:label xml:lang="en">w a c bond coupon</rdfs:label>
	</owl:Class>
	
	<owl:Class rdf:about="&fibo-sec-dbt-bnd;ZeroCouponAndOriginalIssueDiscountBondCallTerms">
		<rdfs:subClassOf rdf:resource="&fibo-sec-dbt-dbti;CallFeature"/>
		<rdfs:subClassOf>
			<owl:Restriction>
				<owl:onProperty rdf:resource="&fibo-fnd-rel-rel;comprises"/>
				<owl:someValuesFrom rdf:resource="&fibo-sec-dbt-bnd;ZeroCouponBondCall"/>
			</owl:Restriction>
		</rdfs:subClassOf>
		<rdfs:label>zero coupon and original issue discount bond call terms</rdfs:label>
		<skos:definition>call feature specific to a zero coupon or original issue discount (OID) bond</skos:definition>
		<fibo-fnd-utl-av:explanatoryNote>Fannie Mae also issues zero-coupon callable debt securities. Zero-coupon notes are debt securities on which no coupon interest is paid to the investor. Rather, the security is purchased at a discounted dollar price and matures at par. If the option on a callable zero-coupon security is exercised, it is redeemed at a higher dollar price than the original issue price. The yield for a callable zero-coupon security is based on the difference between the original discounted price and the principal payment at the call date.</fibo-fnd-utl-av:explanatoryNote>
	</owl:Class>
	
	<owl:Class rdf:about="&fibo-sec-dbt-bnd;ZeroCouponBond">
		<rdfs:subClassOf rdf:resource="&fibo-sec-dbt-bnd;Bond"/>
		<rdfs:subClassOf>
			<owl:Restriction>
				<owl:onProperty rdf:resource="&fibo-sec-dbt-dbti;hasRelativePriceAtMaturity"/>
				<owl:hasValue rdf:resource="&fibo-sec-dbt-dbti;ParValue"/>
			</owl:Restriction>
		</rdfs:subClassOf>
		<rdfs:subClassOf>
			<owl:Restriction>
				<owl:onProperty rdf:resource="&fibo-sec-dbt-bnd;hasOriginalIssueDiscountAmount"/>
				<owl:onClass rdf:resource="&fibo-fnd-acc-cur;MonetaryAmount"/>
				<owl:minQualifiedCardinality rdf:datatype="&xsd;nonNegativeInteger">0</owl:minQualifiedCardinality>
			</owl:Restriction>
		</rdfs:subClassOf>
		<rdfs:subClassOf>
			<owl:Restriction>
				<owl:onProperty rdf:resource="&fibo-sec-dbt-dbti;hasCallFeature"/>
				<owl:someValuesFrom rdf:resource="&fibo-sec-dbt-bnd;ZeroCouponAndOriginalIssueDiscountBondCallTerms"/>
			</owl:Restriction>
		</rdfs:subClassOf>
		<rdfs:subClassOf>
			<owl:Restriction>
				<owl:onProperty rdf:resource="&fibo-sec-dbt-dbti;hasInterestPaymentTerms"/>
				<owl:someValuesFrom rdf:resource="&fibo-sec-dbt-bnd;ZeroCouponTerms"/>
			</owl:Restriction>
		</rdfs:subClassOf>
		<rdfs:label>zero coupon bond</rdfs:label>
		<skos:definition>bond that does not pay interest but is traded at a deep discount, rendering profit at maturity when the bond is redeemed for its full face value</skos:definition>
		<fibo-fnd-utl-av:explanatoryNote>Note that a zero coupon is treated for calculation purposes as a fixed coupon bond with a coupon rate of zero, rather than as a bond without a coupon rate.</fibo-fnd-utl-av:explanatoryNote>
		<fibo-fnd-utl-av:synonym>z-bond</fibo-fnd-utl-av:synonym>
	</owl:Class>
	
	<owl:Class rdf:about="&fibo-sec-dbt-bnd;ZeroCouponBondCall">
		<rdfs:subClassOf rdf:resource="&fibo-sec-dbt-dbti;CallEvent"/>
		<rdfs:subClassOf>
			<owl:Restriction>
				<owl:onProperty rdf:resource="&fibo-sec-dbt-bnd;hasCallRateBasis"/>
				<owl:someValuesFrom rdf:resource="&fibo-sec-dbt-bnd;RateBasisType"/>
			</owl:Restriction>
		</rdfs:subClassOf>
		<rdfs:label>zero coupon bond call</rdfs:label>
		<skos:definition>call event associated with a zero coupon or original issue discount bond</skos:definition>
	</owl:Class>
	
	<owl:Class rdf:about="&fibo-sec-dbt-bnd;ZeroCouponTerms">
		<rdfs:subClassOf rdf:resource="&fibo-sec-dbt-bnd;BondAmortizationPaymentTerms"/>
		<rdfs:subClassOf rdf:resource="&fibo-sec-dbt-bnd;FixedCouponTerms"/>
		<rdfs:subClassOf>
			<owl:Restriction>
				<owl:onProperty rdf:resource="&fibo-fbc-dae-dbt;hasInterestRate"/>
				<owl:hasValue rdf:resource="&fibo-sec-dbt-bnd;ZeroInterestRate"/>
			</owl:Restriction>
		</rdfs:subClassOf>
		<rdfs:label>zero coupon terms</rdfs:label>
		<skos:definition>terms for payment of interest on a zero coupon bond</skos:definition>
	</owl:Class>
	
	<owl:NamedIndividual rdf:about="&fibo-sec-dbt-bnd;ZeroInterestRate">
		<rdf:type rdf:resource="&fibo-fbc-dae-dbt;FixedInterestRate"/>
		<rdfs:label>zero interest rate</rdfs:label>
		<skos:definition>an interest rate of zero (0) percent</skos:definition>
		<fibo-fnd-acc-cur:hasRateValue rdf:datatype="&xsd;decimal">0.00</fibo-fnd-acc-cur:hasRateValue>
	</owl:NamedIndividual>
	
	<owl:DatatypeProperty rdf:about="&fibo-sec-dbt-bnd;baseOffsetBusinessDays">
		<rdfs:label xml:lang="en">base offset business days</rdfs:label>
		<rdfs:domain rdf:resource="&fibo-sec-dbt-bnd;FloatingRateNoteTerms"/>
		<rdfs:range rdf:resource="&xsd;integer"/>
		<skos:definition xml:lang="en">Number of days before the coupon refix date, when the value of the underlying base is to be taken from. Also known as Lookback.</skos:definition>
	</owl:DatatypeProperty>
	
	<owl:ObjectProperty rdf:about="&fibo-sec-dbt-bnd;cap">
		<rdfs:label xml:lang="en">cap</rdfs:label>
		<rdfs:domain rdf:resource="&fibo-sec-dbt-bnd;VariableInterestExpression"/>
		<rdfs:range rdf:resource="&fibo-fnd-utl-val;PercentageValue"/>
	</owl:ObjectProperty>
	
	<owl:DatatypeProperty rdf:about="&fibo-sec-dbt-bnd;capitalizedInterest">
		<rdfs:label xml:lang="en">capitalized interest</rdfs:label>
		<rdfs:domain rdf:resource="&fibo-sec-dbt-bnd;Bond"/>
		<rdfs:range rdf:resource="&xsd;boolean"/>
		<skos:definition xml:lang="en">Whether the interest amount is capitalised until maturity date or paid out at each interest payment date.</skos:definition>
	</owl:DatatypeProperty>
	
	<owl:DatatypeProperty rdf:about="&fibo-sec-dbt-bnd;condition">
		<rdfs:label xml:lang="en">condition</rdfs:label>
		<rdfs:domain rdf:resource="&fibo-sec-dbt-bnd;CouponConditionalTerm"/>
		<rdfs:range rdf:resource="&xsd;string"/>
		<skos:definition xml:lang="en">The condition under which the given coupon is payable. This is stated as text.</skos:definition>
	</owl:DatatypeProperty>
	
	<owl:ObjectProperty rdf:about="&fibo-sec-dbt-bnd;floor">
		<rdfs:label xml:lang="en">floor</rdfs:label>
		<rdfs:domain rdf:resource="&fibo-sec-dbt-bnd;VariableInterestExpression"/>
		<rdfs:range rdf:resource="&fibo-fnd-utl-val;PercentageValue"/>
	</owl:ObjectProperty>
	
	<owl:ObjectProperty rdf:about="&fibo-sec-dbt-bnd;hasAwardDate">
		<rdfs:subPropertyOf rdf:resource="&fibo-fnd-dt-fd;hasDate"/>
		<rdfs:label xml:lang="en">has award date</rdfs:label>
		<rdfs:domain rdf:resource="&fibo-sec-dbt-bnd;MunicipalBond"/>
		<rdfs:range rdf:resource="&fibo-fnd-dt-fd;Date"/>
		<skos:definition xml:lang="en">Date on which bonds are awarded to the lead manager or syndicate on negotiated deals or the date of bidding on competitive deals.</skos:definition>
		<skos:editorialNote xml:lang="en">There are two kinds of award date in municipal securities issuance: verbal award date and formal award date</skos:editorialNote>
		<fibo-fnd-utl-av:synonym xml:lang="en">has sale date</fibo-fnd-utl-av:synonym>
	</owl:ObjectProperty>
	
	<owl:ObjectProperty rdf:about="&fibo-sec-dbt-bnd;hasBondMaturityRegistrar">
		<rdfs:subPropertyOf rdf:resource="&fibo-fnd-agr-ctr;hasThirdParty"/>
		<rdfs:label xml:lang="en">has bond maturity registrar</rdfs:label>
		<rdfs:domain rdf:resource="&fibo-sec-dbt-bnd;Bond"/>
		<rdfs:range rdf:resource="&fibo-sec-dbt-bnd;BondMaturityRegistrar"/>
		<skos:definition xml:lang="en">The person or entity responsible for maintaining records on behalf of the issuer that identify the owners of a registered bond issue.</skos:definition>
	</owl:ObjectProperty>
	
	<owl:ObjectProperty rdf:about="&fibo-sec-dbt-bnd;hasCallPrice">
		<rdfs:subPropertyOf rdf:resource="&fibo-fnd-acc-cur;hasPrice"/>
		<rdfs:label xml:lang="en">has call price</rdfs:label>
		<rdfs:domain rdf:resource="&fibo-sec-dbt-dbti;CallFeature"/>
		<rdfs:range rdf:resource="&fibo-sec-dbt-dbti;CallPrice"/>
		<skos:definition>the amount of the call on the specified call date, typically the sum of par value and the call premium, as specified in the contract</skos:definition>
		<fibo-fnd-utl-av:explanatoryNote>This is the price a bond issuer or preferred stock issuer must pay investors to buy back, or call, all or part of an issue before the maturity date.</fibo-fnd-utl-av:explanatoryNote>
		<fibo-fnd-utl-av:synonym>has redemption price</fibo-fnd-utl-av:synonym>
	</owl:ObjectProperty>
	
	<owl:ObjectProperty rdf:about="&fibo-sec-dbt-bnd;hasCallRateBasis">
		<rdfs:label xml:lang="en">has call rate basis</rdfs:label>
		<rdfs:domain rdf:resource="&fibo-sec-dbt-bnd;ZeroCouponBondCall"/>
		<rdfs:range rdf:resource="&fibo-sec-dbt-bnd;RateBasisType"/>
		<skos:definition xml:lang="en">For each call event on the schedule: whether the rate is expressed as a % of Par or % of CAV. Zero coupon bonds and OID bonds are callable at an accreted value.</skos:definition>
	</owl:ObjectProperty>
	
	<owl:ObjectProperty rdf:about="&fibo-sec-dbt-bnd;hasCallRedemptionType">
		<rdfs:label xml:lang="en">has call redemption type</rdfs:label>
		<rdfs:domain rdf:resource="&fibo-sec-dbt-bnd;PartialCall"/>
		<rdfs:range rdf:resource="&fibo-sec-dbt-bnd;PartialCallAllocation"/>
		<skos:definition xml:lang="en">Whether the call will be executed by Lottery or Pro-Rata.</skos:definition>
	</owl:ObjectProperty>
	
	<owl:ObjectProperty rdf:about="&fibo-sec-dbt-bnd;hasConvertibleDate">
		<rdfs:subPropertyOf rdf:resource="&fibo-fnd-dt-fd;hasDate"/>
		<rdfs:label xml:lang="en">has convertible date</rdfs:label>
		<rdfs:domain rdf:resource="&fibo-sec-dbt-bnd;BondConversionTerms"/>
		<rdfs:range rdf:resource="&fibo-fnd-dt-fd;Date"/>
		<skos:definition>the date on which a bond can be converted into the specified equity security</skos:definition>
	</owl:ObjectProperty>
	
	<owl:ObjectProperty rdf:about="&fibo-sec-dbt-bnd;hasCouponCurrency">
		<rdfs:label xml:lang="en">coupon payment currency</rdfs:label>
		<rdfs:domain rdf:resource="&fibo-sec-dbt-bnd;CouponPaymentTerms"/>
		<rdfs:range rdf:resource="&fibo-fnd-acc-cur;Currency"/>
		<skos:definition xml:lang="en">indicates the currency in which interest payments are to be made</skos:definition>
	</owl:ObjectProperty>
	
	<owl:ObjectProperty rdf:about="&fibo-sec-dbt-bnd;hasEntireOrPartialCallChoice">
		<rdfs:label xml:lang="en">has entire or partial call choice</rdfs:label>
		<rdfs:domain rdf:resource="&fibo-sec-dbt-dbti;CallSchedule"/>
		<rdfs:range rdf:resource="&fibo-sec-dbt-bnd;EntireOrPartialCallChoice"/>
	</owl:ObjectProperty>
	
	<owl:ObjectProperty rdf:about="&fibo-sec-dbt-bnd;hasExerciseType">
		<rdfs:label xml:lang="en">has exercise type</rdfs:label>
		<rdfs:domain rdf:resource="&fibo-sec-dbt-dbti;CallFeature"/>
		<rdfs:range rdf:resource="&fibo-sec-dbt-ex;ExerciseConvention"/>
	</owl:ObjectProperty>
	
	<owl:ObjectProperty rdf:about="&fibo-sec-dbt-bnd;hasExtraordinaryRedemptionProvision">
		<rdfs:subPropertyOf rdf:resource="&fibo-fnd-agr-ctr;hasContractualElement"/>
		<rdfs:label xml:lang="en">has extraordinary redemption provision</rdfs:label>
		<rdfs:domain rdf:resource="&fibo-sec-dbt-dbti;TradableDebtInstrumentRedemptionProvision"/>
		<rdfs:range rdf:resource="&fibo-sec-dbt-bnd;ExtraordinaryRedemptionProvision"/>
		<skos:definition>relates the redemption provision of a debt instrument to one-time redemption provision that may be exercised by the issuer under certain circumstances</skos:definition>
	</owl:ObjectProperty>
	
	<owl:ObjectProperty rdf:about="&fibo-sec-dbt-bnd;hasFinalMaturityDate">
		<rdfs:label>has final maturity date</rdfs:label>
		<rdfs:domain rdf:resource="&fibo-sec-dbt-dbti;TradableDebtInstrumentRedemptionProvision"/>
		<rdfs:range rdf:resource="&fibo-fnd-dt-fd;Date"/>
		<skos:definition>the final payment date of a loan or other financial instrument, at which point the principal (and all remaining interest) is due to be paid</skos:definition>
	</owl:ObjectProperty>
	
	<owl:ObjectProperty rdf:about="&fibo-sec-dbt-bnd;hasFirstCallPrice">
		<rdfs:subPropertyOf rdf:resource="&fibo-sec-dbt-bnd;hasCallPrice"/>
		<rdfs:label xml:lang="en">has first call price</rdfs:label>
		<rdfs:domain rdf:resource="&fibo-sec-dbt-dbti;CallFeature"/>
		<rdfs:range rdf:resource="&fibo-sec-dbt-dbti;CallPrice"/>
		<skos:definition>the amount of the call on the first call date as specified in the call schedule</skos:definition>
	</owl:ObjectProperty>
	
	<owl:ObjectProperty rdf:about="&fibo-sec-dbt-bnd;hasFirstCouponPaymentDate">
		<rdfs:subPropertyOf rdf:resource="&fibo-fnd-dt-fd;hasStartDate"/>
		<rdfs:label xml:lang="en">has first coupon payment date</rdfs:label>
		<rdfs:domain rdf:resource="&fibo-sec-dbt-bnd;CouponPaymentTerms"/>
		<rdfs:range rdf:resource="&fibo-fnd-dt-fd;Date"/>
		<skos:definition xml:lang="en">the first date on which the issuer or its agent expects or commits to make a coupon payment</skos:definition>
		<fibo-fnd-utl-av:explanatoryNote xml:lang="en">The first coupon payment period can be long or short when this date doesn&apos;t coincide with the start of a normal coupon payment period.</fibo-fnd-utl-av:explanatoryNote>
	</owl:ObjectProperty>
	
	<owl:ObjectProperty rdf:about="&fibo-sec-dbt-bnd;hasFirstParCallDate">
		<rdfs:subPropertyOf rdf:resource="&fibo-fnd-dt-fd;hasStartDate"/>
		<rdfs:label>has first par call date</rdfs:label>
		<rdfs:domain rdf:resource="&fibo-sec-dbt-dbti;CallFeature"/>
		<rdfs:range rdf:resource="&fibo-fnd-dt-fd;Date"/>
		<skos:definition>the first date on which the bond may be called at par for redemption</skos:definition>
	</owl:ObjectProperty>
	
	<owl:ObjectProperty rdf:about="&fibo-sec-dbt-bnd;hasFirstParCallPrice">
		<rdfs:subPropertyOf rdf:resource="&fibo-sec-dbt-bnd;hasFirstCallPrice"/>
		<rdfs:label>has first par call price</rdfs:label>
		<rdfs:domain rdf:resource="&fibo-sec-dbt-dbti;CallFeature"/>
		<rdfs:range rdf:resource="&fibo-sec-dbt-dbti;CallPrice"/>
		<skos:definition>the amount of the call on the first par call date as specified in the call schedule</skos:definition>
	</owl:ObjectProperty>
	
	<owl:ObjectProperty rdf:about="&fibo-sec-dbt-bnd;hasFirstPremiumCallDate">
		<rdfs:subPropertyOf rdf:resource="&fibo-fnd-dt-fd;hasStartDate"/>
		<rdfs:label>has first premium call date</rdfs:label>
		<rdfs:domain rdf:resource="&fibo-sec-dbt-dbti;CallFeature"/>
		<rdfs:range rdf:resource="&fibo-fnd-dt-fd;Date"/>
		<skos:definition>the first date on which the bond may be called for redemption at a price above par</skos:definition>
	</owl:ObjectProperty>
	
	<owl:ObjectProperty rdf:about="&fibo-sec-dbt-bnd;hasFirstPremiumCallPrice">
		<rdfs:subPropertyOf rdf:resource="&fibo-sec-dbt-bnd;hasFirstCallPrice"/>
		<rdfs:label>has first premium call price</rdfs:label>
		<rdfs:domain rdf:resource="&fibo-sec-dbt-dbti;CallFeature"/>
		<rdfs:range rdf:resource="&fibo-sec-dbt-dbti;CallPrice"/>
		<skos:definition>the amount of the call on the first call date on which the bond may be called at a price above par as specified in the call schedule</skos:definition>
	</owl:ObjectProperty>
	
	<owl:ObjectProperty rdf:about="&fibo-sec-dbt-bnd;hasFirstPutDate">
		<rdfs:subPropertyOf rdf:resource="&fibo-sec-dbt-bnd;hasPutDate"/>
		<rdfs:label>has first put date</rdfs:label>
		<rdfs:domain rdf:resource="&fibo-sec-dbt-dbti;PutFeature"/>
		<rdfs:range rdf:resource="&fibo-fnd-dt-fd;Date"/>
		<skos:definition>the initial date on which the holder may sell the bond to the issuer prior to maturity</skos:definition>
	</owl:ObjectProperty>
	
	<owl:ObjectProperty rdf:about="&fibo-sec-dbt-bnd;hasFirstPutPrice">
		<rdfs:subPropertyOf rdf:resource="&fibo-fnd-acc-cur;hasPrice"/>
		<rdfs:label xml:lang="en">has first put price</rdfs:label>
		<rdfs:domain rdf:resource="&fibo-sec-dbt-dbti;PutFeature"/>
		<rdfs:range rdf:resource="&fibo-sec-dbt-dbti;PutPrice"/>
		<skos:definition>the initial price at which the holder may sell the bond to the issuer prior to maturity</skos:definition>
	</owl:ObjectProperty>
	
	<owl:ObjectProperty rdf:about="&fibo-sec-dbt-bnd;hasFormalAwardDate">
		<rdfs:subPropertyOf rdf:resource="&fibo-fnd-dt-fd;hasDate"/>
		<rdfs:subPropertyOf rdf:resource="&fibo-sec-dbt-bnd;hasAwardDate"/>
		<rdfs:label xml:lang="en">has formal award date</rdfs:label>
		<rdfs:domain rdf:resource="&fibo-sec-dbt-bnd;MunicipalBond"/>
		<rdfs:range rdf:resource="&fibo-fnd-dt-fd;Date"/>
	</owl:ObjectProperty>
	
	<owl:ObjectProperty rdf:about="&fibo-sec-dbt-bnd;hasMunicipalDebtObligor">
		<rdfs:subPropertyOf rdf:resource="&fibo-fnd-agr-ctr;hasThirdParty"/>
		<rdfs:label xml:lang="en">has municipal debt obligor</rdfs:label>
		<rdfs:domain rdf:resource="&fibo-sec-dbt-bnd;MunicipalSecurity"/>
		<rdfs:range rdf:resource="&fibo-sec-dbt-bnd;MunicipalDebtObligor"/>
	</owl:ObjectProperty>
	
	<owl:ObjectProperty rdf:about="&fibo-sec-dbt-bnd;hasMunicipalTrustee">
		<rdfs:subPropertyOf rdf:resource="&fibo-fnd-agr-ctr;hasThirdParty"/>
		<rdfs:label xml:lang="en">has municipal trustee</rdfs:label>
		<rdfs:domain rdf:resource="&fibo-sec-dbt-bnd;MunicipalBond"/>
		<rdfs:range rdf:resource="&fibo-sec-dbt-bnd;MunicipalTrustee"/>
		<skos:definition xml:lang="en">The financial institution with trust powers, designated by the issuer or borrower, that acts, pursuant to a bond contract, in a fiduciary capacity for the benefit of the bondholders in enforcing the terms of the bond contract.</skos:definition>
	</owl:ObjectProperty>
	
	<owl:ObjectProperty rdf:about="&fibo-sec-dbt-bnd;hasMunicipalUse">
		<rdfs:label xml:lang="en">has municipal use</rdfs:label>
		<rdfs:domain rdf:resource="&fibo-sec-dbt-bnd;MunicipalSecurity"/>
		<rdfs:range rdf:resource="&fibo-sec-dbt-bnd;MunicipalDebtFundsUsage"/>
		<skos:definition xml:lang="en">the application of funds in connection with a new issue of municipal securities</skos:definition>
	</owl:ObjectProperty>
	
	<owl:ObjectProperty rdf:about="&fibo-sec-dbt-bnd;hasOriginalIssueDiscountAmount">
		<rdfs:label xml:lang="en">has original issue discount amount</rdfs:label>
		<rdfs:domain rdf:resource="&fibo-sec-dbt-bnd;ZeroCouponBond"/>
		<rdfs:range rdf:resource="&fibo-fnd-acc-cur;MonetaryAmount"/>
		<skos:definition xml:lang="en">the difference between the stated redemption price at maturity and the issue price</skos:definition>
	</owl:ObjectProperty>
	
	<owl:ObjectProperty rdf:about="&fibo-sec-dbt-bnd;hasPercentage">
		<rdfs:label xml:lang="en">has percentage</rdfs:label>
		<rdfs:domain rdf:resource="&fibo-sec-dbt-bnd;PartialCallAllocation"/>
		<rdfs:range rdf:resource="&fibo-fnd-utl-val;PercentageValue"/>
	</owl:ObjectProperty>
	
	<owl:ObjectProperty rdf:about="&fibo-sec-dbt-bnd;hasPublishedSinkingFundAmortizationTermsDescription">
		<rdfs:label xml:lang="en">has published sinking fund amortization terms description</rdfs:label>
		<rdfs:domain rdf:resource="&fibo-sec-dbt-bnd;BondWithPublishedSinkingFund"/>
		<rdfs:range rdf:resource="&fibo-sec-dbt-bnd;SinkingFundAmortizationTerms"/>
	</owl:ObjectProperty>
	
	<owl:ObjectProperty rdf:about="&fibo-sec-dbt-bnd;hasPutDate">
		<rdfs:subPropertyOf rdf:resource="&fibo-fnd-dt-fd;hasDate"/>
		<rdfs:label>has put date</rdfs:label>
		<rdfs:domain rdf:resource="&fibo-sec-dbt-dbti;PutFeature"/>
		<rdfs:range rdf:resource="&fibo-fnd-dt-fd;Date"/>
		<skos:definition>the date on which a security is subject to optional or mandatory redemption by the bond holder</skos:definition>
	</owl:ObjectProperty>
	
	<owl:ObjectProperty rdf:about="&fibo-sec-dbt-bnd;hasPutFrequency">
		<rdfs:label>has put frequency</rdfs:label>
		<rdfs:domain rdf:resource="&fibo-sec-dbt-dbti;PutFeature"/>
		<rdfs:range rdf:resource="&fibo-fnd-dt-fd;RecurrenceInterval"/>
		<skos:definition>indicates the frequency of the tender or put period</skos:definition>
	</owl:ObjectProperty>
	
	<owl:ObjectProperty rdf:about="&fibo-sec-dbt-bnd;hasRemarketingAgent">
		<rdfs:subPropertyOf rdf:resource="&fibo-fnd-agr-ctr;hasThirdParty"/>
		<rdfs:label xml:lang="en">has remarketing agent</rdfs:label>
		<rdfs:domain rdf:resource="&fibo-sec-dbt-bnd;MunicipalSecurity"/>
		<rdfs:range rdf:resource="&fibo-sec-dbt-bnd;MunicipalDebtRemarketingAgent"/>
		<skos:definition xml:lang="en">The municipal securities dealer responsible for reselling to investors securities (such as variable rate demand obligations and other tender option bonds) that have been tendered for purchase by their owner.</skos:definition>
	</owl:ObjectProperty>
	
	<owl:ObjectProperty rdf:about="&fibo-sec-dbt-bnd;hasVerbalAwardDate">
		<rdfs:subPropertyOf rdf:resource="&fibo-sec-dbt-bnd;hasAwardDate"/>
		<rdfs:label xml:lang="en">has verbal award date</rdfs:label>
		<rdfs:domain rdf:resource="&fibo-sec-dbt-bnd;MunicipalBond"/>
		<rdfs:range rdf:resource="&fibo-fnd-dt-fd;Date"/>
		<skos:definition xml:lang="en">has a date on which ...</skos:definition>
	</owl:ObjectProperty>
	
	<owl:DatatypeProperty rdf:about="&fibo-sec-dbt-bnd;isBankQualified">
		<rdfs:label xml:lang="en">is bank qualified</rdfs:label>
		<rdfs:domain rdf:resource="&fibo-sec-dbt-bnd;MunicipalBond"/>
		<rdfs:range rdf:resource="&xsd;boolean"/>
		<skos:definition xml:lang="en">Designation given to a public purpose bond offering by the issuer if it reasonably expects to issue in the calendar year of such offering no more than $10 million ($30 million for bonds issued in 2009-2010) of bonds of the type required to be included in making such calculation under section 265(b)(3) of the IRS tax code. When purchased by a commercial bank for its portfolio, the bank may deduct a portion of the interest cost of carry for the position. A bond that is bank qualified is also known as a “qualified tax-exempt obligation.</skos:definition>
	</owl:DatatypeProperty>
	
	<owl:ObjectProperty rdf:about="&fibo-sec-dbt-bnd;isBasedOn">
		<rdfs:label xml:lang="en">is based on</rdfs:label>
		<rdfs:domain rdf:resource="&fibo-sec-dbt-bnd;IndexLinkedSecurity"/>
		<rdfs:range rdf:resource="&fibo-ind-ind-ind;MarketRate"/>
	</owl:ObjectProperty>
	
	<owl:ObjectProperty rdf:about="&fibo-sec-dbt-bnd;issuedDebtAmount">
		<rdfs:label xml:lang="en">issued debt amount</rdfs:label>
		<rdfs:domain rdf:resource="&fibo-sec-dbt-bnd;VariableDebtPrincipal"/>
		<rdfs:range rdf:resource="&fibo-fnd-acc-cur;MonetaryAmount"/>
	</owl:ObjectProperty>
	
	<owl:DatatypeProperty rdf:about="&fibo-sec-dbt-bnd;legalOpinion">
		<rdfs:label xml:lang="en">legal opinion</rdfs:label>
		<rdfs:domain rdf:resource="&fibo-sec-dbt-bnd;MunicipalBond"/>
		<rdfs:range rdf:resource="&xsd;boolean"/>
		<skos:definition xml:lang="en">Whether legal opinion exists for municipal securities.</skos:definition>
	</owl:DatatypeProperty>
	
	<owl:ObjectProperty rdf:about="&fibo-sec-dbt-bnd;lockoutPeriod">
		<rdfs:label xml:lang="en">lockout period</rdfs:label>
		<rdfs:domain rdf:resource="&fibo-sec-dbt-dbti;CallFeature"/>
		<rdfs:range rdf:resource="&fibo-fnd-dt-fd;DatePeriod"/>
		<skos:definition xml:lang="en">The lockout period refers to the amount of time for which a callable security cannot be called and only interest coupon payments are received by the security holder. For example, with a 10-year noncall 3-year (&quot;10nc3&quot;) debt security, the security cannot be called for the first three years.</skos:definition>
	</owl:ObjectProperty>
	
	<owl:ObjectProperty rdf:about="&fibo-sec-dbt-bnd;makeWholeCallBasisPointSpread">
		<rdfs:label xml:lang="en">make whole call basis point spread</rdfs:label>
		<rdfs:domain rdf:resource="&fibo-sec-dbt-bnd;MakeWholeCall"/>
		<rdfs:range rdf:resource="&fibo-fnd-utl-val;PercentageValue"/>
	</owl:ObjectProperty>
	
	<owl:DatatypeProperty rdf:about="&fibo-sec-dbt-bnd;makeWholeTreasuryItem">
		<rdfs:label xml:lang="en">make whole treasury item</rdfs:label>
		<rdfs:domain rdf:resource="&fibo-sec-dbt-bnd;MakeWholeCall"/>
		<rdfs:range rdf:resource="&xsd;string"/>
	</owl:DatatypeProperty>
	
	<owl:DatatypeProperty rdf:about="&fibo-sec-dbt-bnd;mandatory">
		<rdfs:label xml:lang="en">mandatory</rdfs:label>
		<rdfs:domain rdf:resource="&fibo-sec-dbt-bnd;SinkingFundAmortizationTerms"/>
		<rdfs:range rdf:resource="&xsd;boolean"/>
		<skos:definition xml:lang="en">Whether the SF is mandatory or conditional on some event (No means conditional)</skos:definition>
	</owl:DatatypeProperty>
	
	<owl:DatatypeProperty rdf:about="&fibo-sec-dbt-bnd;mandatoryPut">
		<rdfs:label>mandatory put</rdfs:label>
		<rdfs:domain rdf:resource="&fibo-sec-dbt-dbti;PutFeature"/>
		<rdfs:range rdf:resource="&xsd;boolean"/>
		<skos:definition>Whether the redemption prior to maturity date feature is Mandatory to the bond holder. If No, then this is optional.</skos:definition>
	</owl:DatatypeProperty>
	
	<owl:DatatypeProperty rdf:about="&fibo-sec-dbt-bnd;mandatorySinkingFund">
		<rdfs:label xml:lang="en">mandatory sinking fund</rdfs:label>
		<rdfs:label>mandatory sinking fund</rdfs:label>
		<rdfs:domain rdf:resource="&fibo-sec-dbt-bnd;MandatorySinkingFundTerms"/>
		<rdfs:domain rdf:resource="&fibo-sec-dbt-dbti;CallFeature"/>
		<rdfs:range rdf:resource="&xsd;boolean"/>
		<skos:definition>Whether there is a Mandatory Sinking fund feature.</skos:definition>
		<skos:definition xml:lang="en">Yes indicates there is a Mandatory Sinking fund feature.</skos:definition>
	</owl:DatatypeProperty>
	
	<owl:DatatypeProperty rdf:about="&fibo-sec-dbt-bnd;naked">
		<rdfs:label xml:lang="en">naked</rdfs:label>
		<rdfs:domain rdf:resource="&fibo-sec-dbt-bnd;Debenture"/>
		<rdfs:range rdf:resource="&xsd;boolean"/>
		<skos:definition xml:lang="en">Whether the debenture is unsecured (Naked = Yes) or is secured (Naked = No).</skos:definition>
	</owl:DatatypeProperty>
	
	<owl:DatatypeProperty rdf:about="&fibo-sec-dbt-bnd;paysVariableCoupon">
		<rdfs:label xml:lang="en">pays variable coupon</rdfs:label>
		<rdfs:domain rdf:resource="&fibo-sec-dbt-bnd;InflationBondInterestPaymentTerms"/>
		<rdfs:range rdf:resource="&xsd;boolean"/>
		<skos:definition xml:lang="en">Whether the interest payable on the Inflation Bond is variable with reference to the Factor. If Yes, then the terms include an Inflation Bond Variable Coupon. If No, then the terms may be any coupon or set of coupons, by inheritance of this fact from the parent class of Bond Coupon terms.</skos:definition>
	</owl:DatatypeProperty>
	
	<owl:ObjectProperty rdf:about="&fibo-sec-dbt-bnd;premium">
		<rdfs:label xml:lang="en">premium</rdfs:label>
		<rdfs:domain rdf:resource="&fibo-sec-dbt-dbti;CallFeature"/>
		<rdfs:range rdf:resource="&fibo-fnd-acc-cur;MonetaryAmount"/>
		<skos:definition xml:lang="en">A premium paid to the bond owner when the bond is called.</skos:definition>
	</owl:ObjectProperty>
	
	<owl:DatatypeProperty rdf:about="&fibo-sec-dbt-bnd;proRated">
		<rdfs:label>pro rated</rdfs:label>
		<rdfs:domain rdf:resource="&fibo-fbc-dae-dbt;InterestPaymentTerms"/>
		<rdfs:range rdf:resource="&xsd;boolean"/>
		<skos:definition>Whether the coupon is pro rated to the actual number of days in the payment period versus the number of payment periods.</skos:definition>
	</owl:DatatypeProperty>
	
	<owl:ObjectProperty rdf:about="&fibo-sec-dbt-bnd;redemptionAmount">
		<rdfs:label xml:lang="en">redemption amount</rdfs:label>
		<rdfs:domain rdf:resource="&fibo-sec-dbt-bnd;RedemptionPayment"/>
		<rdfs:range rdf:resource="&fibo-fnd-acc-cur;MonetaryAmount"/>
		<skos:definition xml:lang="en">The amount of the principal paid with this redemption payment.</skos:definition>
	</owl:ObjectProperty>
	
	<owl:DatatypeProperty rdf:about="&fibo-sec-dbt-bnd;resetDateOffsetDays">
		<rdfs:label xml:lang="en">reset date offset days</rdfs:label>
		<rdfs:domain rdf:resource="&fibo-sec-dbt-bnd;VariableCouponTerms"/>
		<rdfs:range rdf:resource="&xsd;integer"/>
		<skos:definition xml:lang="en">Number of days from the Coupon Payment Date that the Coupon Rate is reset. Offset - Relative date e.g. 2 days before Rate rest may be the Fixing date. Payment is separate from this, so this is an Accrual term. Payment dates may also be specified relative to.</skos:definition>
	</owl:DatatypeProperty>
	
	<owl:ObjectProperty rdf:about="&fibo-sec-dbt-bnd;specialRecordDate">
		<rdfs:label xml:lang="en">special record date</rdfs:label>
		<rdfs:domain rdf:resource="&fibo-sec-dbt-bnd;CouponPaymentTerms"/>
		<rdfs:range rdf:resource="&fibo-fnd-dt-fd;Date"/>
		<skos:definition xml:lang="en">The record date associated with an odd first interest payment date that occurs before the start of the normal accrual cycle.</skos:definition>
	</owl:ObjectProperty>
	
	<owl:ObjectProperty rdf:about="&fibo-sec-dbt-bnd;specifiesIndexParameter">
		<rdfs:label xml:lang="en">specifies index parameter</rdfs:label>
		<rdfs:domain rdf:resource="&fibo-sec-dbt-bnd;IndexLinkedPrincipalDeterminationTerms"/>
		<rdfs:range rdf:resource="&fibo-ind-ei-ei;InflationRate"/>
		<skos:definition xml:lang="en">The term specified in the formula for determination of principal paydown amounts.</skos:definition>
	</owl:ObjectProperty>
	
	<owl:DatatypeProperty rdf:about="&fibo-sec-dbt-bnd;superSinker">
		<rdfs:label xml:lang="en">super sinker</rdfs:label>
		<rdfs:domain rdf:resource="&fibo-sec-dbt-bnd;MandatorySinkingFundTerms"/>
		<rdfs:range rdf:resource="&xsd;boolean"/>
		<skos:definition xml:lang="en">A colloquial term for a term maturity, usually from a single family mortgage revenue issue with several term maturities, that will be the first to be called from a sinking fund into which all proceeds from prepayments of mortgages financed by the issue are deposited.  The maturity&apos;s priority status under the call provisions means that it is likely to be redeemed in its entirety well before the stated maturity date.</skos:definition>
	</owl:DatatypeProperty>

</rdf:RDF>