<?xml version="1.0" encoding="UTF-8"?>
<!DOCTYPE rdf:RDF [
	<!ENTITY dct "http://purl.org/dc/terms/">
	<!ENTITY fibo-fbc-fi-fi "https://spec.edmcouncil.org/fibo/ontology/FBC/FinancialInstruments/FinancialInstruments/">
	<!ENTITY fibo-fnd-agr-ctr "https://spec.edmcouncil.org/fibo/ontology/FND/Agreements/Contracts/">
	<!ENTITY fibo-fnd-dt-bd "https://spec.edmcouncil.org/fibo/ontology/FND/DatesAndTimes/BusinessDates/">
	<!ENTITY fibo-fnd-dt-fd "https://spec.edmcouncil.org/fibo/ontology/FND/DatesAndTimes/FinancialDates/">
	<!ENTITY fibo-fnd-rel-rel "https://spec.edmcouncil.org/fibo/ontology/FND/Relations/Relations/">
	<!ENTITY fibo-fnd-utl-av "https://spec.edmcouncil.org/fibo/ontology/FND/Utilities/AnnotationVocabulary/">
	<!ENTITY fibo-sec-dbt-ex "https://spec.edmcouncil.org/fibo/ontology/SEC/Debt/ExerciseConventions/">
	<!ENTITY owl "http://www.w3.org/2002/07/owl#">
	<!ENTITY rdf "http://www.w3.org/1999/02/22-rdf-syntax-ns#">
	<!ENTITY rdfs "http://www.w3.org/2000/01/rdf-schema#">
	<!ENTITY skos "http://www.w3.org/2004/02/skos/core#">
	<!ENTITY sm "http://www.omg.org/techprocess/ab/SpecificationMetadata/">
	<!ENTITY xsd "http://www.w3.org/2001/XMLSchema#">
]>
<rdf:RDF xml:base="https://spec.edmcouncil.org/fibo/ontology/SEC/Debt/ExerciseConventions/"
	xmlns:dct="http://purl.org/dc/terms/"
	xmlns:fibo-fbc-fi-fi="https://spec.edmcouncil.org/fibo/ontology/FBC/FinancialInstruments/FinancialInstruments/"
	xmlns:fibo-fnd-agr-ctr="https://spec.edmcouncil.org/fibo/ontology/FND/Agreements/Contracts/"
	xmlns:fibo-fnd-dt-bd="https://spec.edmcouncil.org/fibo/ontology/FND/DatesAndTimes/BusinessDates/"
	xmlns:fibo-fnd-dt-fd="https://spec.edmcouncil.org/fibo/ontology/FND/DatesAndTimes/FinancialDates/"
	xmlns:fibo-fnd-rel-rel="https://spec.edmcouncil.org/fibo/ontology/FND/Relations/Relations/"
	xmlns:fibo-fnd-utl-av="https://spec.edmcouncil.org/fibo/ontology/FND/Utilities/AnnotationVocabulary/"
	xmlns:fibo-sec-dbt-ex="https://spec.edmcouncil.org/fibo/ontology/SEC/Debt/ExerciseConventions/"
	xmlns:owl="http://www.w3.org/2002/07/owl#"
	xmlns:rdf="http://www.w3.org/1999/02/22-rdf-syntax-ns#"
	xmlns:rdfs="http://www.w3.org/2000/01/rdf-schema#"
	xmlns:skos="http://www.w3.org/2004/02/skos/core#"
	xmlns:sm="http://www.omg.org/techprocess/ab/SpecificationMetadata/"
	xmlns:xsd="http://www.w3.org/2001/XMLSchema#">
	
	<owl:Ontology rdf:about="https://spec.edmcouncil.org/fibo/ontology/SEC/Debt/ExerciseConventions/">
		<rdfs:label xml:lang="en">Exercise Conventions Ontology</rdfs:label>
		<dct:abstract>This ontology defines the various kinds of exercise conventions that are common to debt and options instruments. They are distinguished primarily in terms of the date period during which an optional contract clause may be exercised.</dct:abstract>
		<dct:license rdf:datatype="&xsd;anyURI">http://opensource.org/licenses/MIT</dct:license>
		<sm:contentLanguage rdf:resource="http://www.w3.org/standards/techs/owl#w3c_all"/>
		<sm:copyright>Copyright (c) 2018-2019 EDM Council, Inc.</sm:copyright>
		<sm:dependsOn rdf:datatype="&xsd;anyURI">https://spec.edmcouncil.org/fibo/ontology/FBC/</sm:dependsOn>
		<sm:dependsOn rdf:datatype="&xsd;anyURI">https://spec.edmcouncil.org/fibo/ontology/FND/</sm:dependsOn>
		<sm:fileAbbreviation>fibo-sec-dbt-ex</sm:fileAbbreviation>
		<sm:filename>ExerciseConventions.rdf</sm:filename>
		<owl:imports rdf:resource="https://spec.edmcouncil.org/fibo/ontology/FBC/FinancialInstruments/FinancialInstruments/"/>
		<owl:imports rdf:resource="https://spec.edmcouncil.org/fibo/ontology/FND/Agreements/Contracts/"/>
		<owl:imports rdf:resource="https://spec.edmcouncil.org/fibo/ontology/FND/DatesAndTimes/BusinessDates/"/>
		<owl:imports rdf:resource="https://spec.edmcouncil.org/fibo/ontology/FND/DatesAndTimes/FinancialDates/"/>
		<owl:imports rdf:resource="https://spec.edmcouncil.org/fibo/ontology/FND/Relations/Relations/"/>
		<owl:imports rdf:resource="https://spec.edmcouncil.org/fibo/ontology/FND/Utilities/AnnotationVocabulary/"/>
		<owl:versionIRI rdf:resource="https://spec.edmcouncil.org/fibo/ontology/SEC/20190501/Debt/ExerciseConventions/"/>
		<skos:changeNote>The https://spec.edmcouncil.org/fibo/ontology/SEC/20190101/Debt/ExerciseConventions.rdf version of this ontology was added to support integration of Bonds and Options in SEC and DER, respectively.</skos:changeNote>
		<skos:changeNote>The https://spec.edmcouncil.org/fibo/ontology/SEC/20190101/Debt/ExerciseConventions.rdf version of this ontology was modified to add the hasExerciseTerms property.</skos:changeNote>
		<fibo-fnd-utl-av:hasMaturityLevel rdf:resource="&fibo-fnd-utl-av;Release"/>
	</owl:Ontology>
	
	<owl:NamedIndividual rdf:about="&fibo-sec-dbt-ex;AmericanExerciseConvention">
		<rdf:type rdf:resource="&fibo-sec-dbt-ex;ExerciseConvention"/>
		<rdfs:label xml:lang="en">American exercise convention</rdfs:label>
		<skos:definition xml:lang="en">exercise convention that stipulates that an option may be exercised anytime between the purchase date and date of expiration</skos:definition>
	</owl:NamedIndividual>
	
	<owl:Class rdf:about="&fibo-sec-dbt-ex;AmericanExerciseTerms">
		<rdfs:subClassOf rdf:resource="&fibo-sec-dbt-ex;ExerciseTerms"/>
		<rdfs:subClassOf>
			<owl:Restriction>
				<owl:onProperty rdf:resource="&fibo-fnd-rel-rel;uses"/>
				<owl:hasValue rdf:resource="&fibo-sec-dbt-ex;AmericanExerciseConvention"/>
			</owl:Restriction>
		</rdfs:subClassOf>
		<rdfs:subClassOf>
			<owl:Restriction>
				<owl:onProperty rdf:resource="&fibo-sec-dbt-ex;hasExerciseWindow"/>
				<owl:someValuesFrom rdf:resource="&fibo-fnd-dt-fd;DatePeriod"/>
			</owl:Restriction>
		</rdfs:subClassOf>
		<rdfs:label xml:lang="en">American exercise terms</rdfs:label>
		<owl:disjointWith rdf:resource="&fibo-sec-dbt-ex;BermudanExerciseTerms"/>
		<owl:disjointWith rdf:resource="&fibo-sec-dbt-ex;EuropeanExerciseTerms"/>
		<skos:definition xml:lang="en">exercise terms that stipulate that an option may be exercised anytime between the purchase date and date of expiration</skos:definition>
		<fibo-fnd-utl-av:explanatoryNote xml:lang="en">Under certain circumstances, early exercise may be advantageous to the option holder.</fibo-fnd-utl-av:explanatoryNote>
	</owl:Class>
	
	<owl:NamedIndividual rdf:about="&fibo-sec-dbt-ex;BermudanExerciseConvention">
		<rdf:type rdf:resource="&fibo-sec-dbt-ex;ExerciseConvention"/>
		<rdfs:label xml:lang="en">Bermudan exercise convention</rdfs:label>
		<skos:definition xml:lang="en">exercise convention that stipulates that an option may be exercised anytime between the purchase date and date of expiration</skos:definition>
	</owl:NamedIndividual>
	
	<owl:Class rdf:about="&fibo-sec-dbt-ex;BermudanExerciseTerms">
		<rdfs:subClassOf rdf:resource="&fibo-sec-dbt-ex;ExerciseTerms"/>
		<rdfs:subClassOf>
			<owl:Restriction>
				<owl:onProperty rdf:resource="&fibo-fnd-rel-rel;uses"/>
				<owl:hasValue rdf:resource="&fibo-sec-dbt-ex;BermudanExerciseConvention"/>
			</owl:Restriction>
		</rdfs:subClassOf>
		<rdfs:subClassOf>
			<owl:Restriction>
				<owl:onProperty rdf:resource="&fibo-sec-dbt-ex;hasExerciseDate"/>
				<owl:someValuesFrom rdf:resource="&fibo-fnd-dt-fd;ExplicitDate"/>
			</owl:Restriction>
		</rdfs:subClassOf>
		<rdfs:subClassOf>
			<owl:Restriction>
				<owl:onProperty rdf:resource="&fibo-sec-dbt-ex;hasExerciseWindow"/>
				<owl:someValuesFrom rdf:resource="&fibo-fnd-dt-fd;DatePeriod"/>
			</owl:Restriction>
		</rdfs:subClassOf>
		<rdfs:label xml:lang="en">Bermudan exercise terms</rdfs:label>
		<owl:disjointWith rdf:resource="&fibo-sec-dbt-ex;EuropeanExerciseTerms"/>
		<skos:definition xml:lang="en">exercise terms that stipulate that an option may only be exercised on predetermined dates within some exercise window, often on one day each month or at the date of expiration</skos:definition>
		<fibo-fnd-utl-av:explanatoryNote xml:lang="en">The Bermuda option is named as such because its exercise dates are more flexible than European options and less flexible than American options. Thus, it is in the middle, just like Bermuda is between Europe and America. Bermuda options are also referred to as Mid-Atlantic, Quasi American, or Semi-American options.</fibo-fnd-utl-av:explanatoryNote>
	</owl:Class>
	
	<owl:NamedIndividual rdf:about="&fibo-sec-dbt-ex;CanaryExerciseConvention">
		<rdf:type rdf:resource="&fibo-sec-dbt-ex;ExerciseConvention"/>
		<rdfs:label xml:lang="en">canary exercise convention</rdfs:label>
		<skos:definition xml:lang="en">exercise/call convention that stipulates that an option may only be exercised on predetermined dates until the first step is reached, but not after that point</skos:definition>
	</owl:NamedIndividual>
	
	<owl:Class rdf:about="&fibo-sec-dbt-ex;CanaryExerciseTerms">
		<rdfs:subClassOf rdf:resource="&fibo-sec-dbt-ex;BermudanExerciseTerms"/>
		<rdfs:subClassOf>
			<owl:Restriction>
				<owl:onProperty rdf:resource="&fibo-fnd-rel-rel;uses"/>
				<owl:hasValue rdf:resource="&fibo-sec-dbt-ex;CanaryExerciseConvention"/>
			</owl:Restriction>
		</rdfs:subClassOf>
		<rdfs:label xml:lang="en">canary exercise terms</rdfs:label>
		<skos:definition xml:lang="en">exercise terms that stipulate that an option may only be exercised on predetermined dates until the first step is reached, but not after that point</skos:definition>
	</owl:Class>
	
	<owl:NamedIndividual rdf:about="&fibo-sec-dbt-ex;EuropeanExerciseConvention">
		<rdf:type rdf:resource="&fibo-sec-dbt-ex;ExerciseConvention"/>
		<rdfs:label xml:lang="en">European exercise convention</rdfs:label>
		<skos:definition xml:lang="en">exercise convention that stipulates that an option may only be exercised at the date of expiration</skos:definition>
	</owl:NamedIndividual>
	
	<owl:Class rdf:about="&fibo-sec-dbt-ex;EuropeanExerciseTerms">
		<rdfs:subClassOf rdf:resource="&fibo-sec-dbt-ex;ExerciseTerms"/>
		<rdfs:subClassOf>
			<owl:Restriction>
				<owl:onProperty rdf:resource="&fibo-fnd-rel-rel;uses"/>
				<owl:hasValue rdf:resource="&fibo-sec-dbt-ex;EuropeanExerciseConvention"/>
			</owl:Restriction>
		</rdfs:subClassOf>
		<rdfs:subClassOf>
			<owl:Restriction>
				<owl:onProperty rdf:resource="&fibo-sec-dbt-ex;hasExerciseDate"/>
				<owl:onClass rdf:resource="&fibo-fnd-dt-fd;ExplicitDate"/>
				<owl:qualifiedCardinality rdf:datatype="&xsd;nonNegativeInteger">1</owl:qualifiedCardinality>
			</owl:Restriction>
		</rdfs:subClassOf>
		<rdfs:label xml:lang="en">European exercise terms</rdfs:label>
		<skos:definition xml:lang="en">exercise terms that stipulate that an option may only be exercised at the date of expiration</skos:definition>
	</owl:Class>
	
	<owl:Class rdf:about="&fibo-sec-dbt-ex;ExerciseConvention">
		<rdfs:subClassOf rdf:resource="&fibo-fnd-dt-bd;Convention"/>
		<rdfs:label xml:lang="en">exercise convention</rdfs:label>
		<skos:definition xml:lang="en">convention that determines when the holder or future holder of an option can implement the rights defined in the option</skos:definition>
	</owl:Class>
	
	<owl:Class rdf:about="&fibo-sec-dbt-ex;ExerciseTerms">
		<rdfs:subClassOf rdf:resource="&fibo-fnd-agr-ctr;ContractualCommitment"/>
		<rdfs:subClassOf>
			<owl:Restriction>
				<owl:onProperty rdf:resource="&fibo-fnd-rel-rel;uses"/>
				<owl:someValuesFrom rdf:resource="&fibo-sec-dbt-ex;ExerciseConvention"/>
			</owl:Restriction>
		</rdfs:subClassOf>
		<rdfs:label xml:lang="en">exercise terms</rdfs:label>
		<skos:definition xml:lang="en">contract terms specific to the conditions, conventions and other stipulations related to the exercise of an option</skos:definition>
	</owl:Class>
	
	<owl:ObjectProperty rdf:about="&fibo-sec-dbt-ex;hasExerciseDate">
		<rdfs:subPropertyOf rdf:resource="&fibo-fnd-dt-fd;hasExplicitDate"/>
		<rdfs:label xml:lang="en">has exercise date</rdfs:label>
		<rdfs:range rdf:resource="&fibo-fnd-dt-fd;ExplicitDate"/>
		<skos:definition xml:lang="en">indicates a date on which an option may be exercised as specified in the terms of the contract</skos:definition>
	</owl:ObjectProperty>
	
	<owl:ObjectProperty rdf:about="&fibo-sec-dbt-ex;hasExerciseTerms">
		<rdfs:subPropertyOf rdf:resource="&fibo-fnd-agr-ctr;hasContractualElement"/>
		<rdfs:label xml:lang="en">has exercise terms</rdfs:label>
		<rdfs:domain rdf:resource="&fibo-fbc-fi-fi;Option"/>
		<rdfs:range rdf:resource="&fibo-sec-dbt-ex;ExerciseTerms"/>
		<skos:definition xml:lang="en">links an option contract to any exercise terms that are specified therein</skos:definition>
	</owl:ObjectProperty>
	
	<owl:ObjectProperty rdf:about="&fibo-sec-dbt-ex;hasExerciseWindow">
		<rdfs:label xml:lang="en">has exercise window</rdfs:label>
		<rdfs:range rdf:resource="&fibo-fnd-dt-fd;DatePeriod"/>
		<skos:definition xml:lang="en">indicates a period of time during which the option may be exercised as specified in the terms of the contract</skos:definition>
	</owl:ObjectProperty>

</rdf:RDF>