<?xml version="1.0" encoding="UTF-8"?>
<!DOCTYPE rdf:RDF [
	<!ENTITY fibo-fnd-bus-bg "https://spec.edmcouncil.org/fibo/FND/BusinessExt/BusinessGoals/">
	<!ENTITY fibo-fnd-gao-gl "https://spec.edmcouncil.org/fibo/FND/GoalsAndObjectives/Goals/">
	<!ENTITY fibo-fnd-utl-av "https://spec.edmcouncil.org/fibo/FND/Utilities/AnnotationVocabulary/">
	<!ENTITY owl "http://www.w3.org/2002/07/owl#">
	<!ENTITY rdf "http://www.w3.org/1999/02/22-rdf-syntax-ns#">
	<!ENTITY rdfs "http://www.w3.org/2000/01/rdf-schema#">
	<!ENTITY skos "http://www.w3.org/2004/02/skos/core#">
	<!ENTITY xsd "http://www.w3.org/2001/XMLSchema#">
]>
<rdf:RDF xml:base="https://spec.edmcouncil.org/fibo/FND/BusinessExt/BusinessGoals/"
	xmlns:fibo-fnd-bus-bg="https://spec.edmcouncil.org/fibo/FND/BusinessExt/BusinessGoals/"
	xmlns:fibo-fnd-gao-gl="https://spec.edmcouncil.org/fibo/FND/GoalsAndObjectives/Goals/"
	xmlns:fibo-fnd-utl-av="https://spec.edmcouncil.org/fibo/FND/Utilities/AnnotationVocabulary/"
	xmlns:owl="http://www.w3.org/2002/07/owl#"
	xmlns:rdf="http://www.w3.org/1999/02/22-rdf-syntax-ns#"
	xmlns:rdfs="http://www.w3.org/2000/01/rdf-schema#"
	xmlns:skos="http://www.w3.org/2004/02/skos/core#"
	xmlns:xsd="http://www.w3.org/2001/XMLSchema#">
	
	<owl:Ontology rdf:about="https://spec.edmcouncil.org/fibo/FND/BusinessExt/BusinessGoals/">
		<rdfs:label xml:lang="en">BusinessGoals</rdfs:label>
		<owl:imports rdf:resource="http://www.w3.org/2004/02/skos/core"/>
		<owl:imports rdf:resource="https://spec.edmcouncil.org/fibo/FND/GoalsAndObjectives/Goals/"/>
		<owl:imports rdf:resource="https://spec.edmcouncil.org/fibo/FND/Utilities/AnnotationVocabulary/"/>
		<owl:versionIRI rdf:resource="https://spec.edmcouncil.org/fibo/FND/BusinessExt/BusinessGoals/"/>
		<fibo-fnd-utl-av:hasMaturityLevel rdf:resource="&fibo-fnd-utl-av;Informative"/>
	</owl:Ontology>
	
	<owl:Class rdf:about="&fibo-fnd-bus-bg;BusinessGoal">
		<rdfs:subClassOf rdf:resource="&fibo-fnd-gao-gl;Goal"/>
		<rdfs:label xml:lang="en">business goal</rdfs:label>
		<skos:definition xml:lang="en">A Goal is a state or condition of the enterprise to be brought about or sustained through appropriate Means.</skos:definition>
	</owl:Class>
	
	<owl:Class rdf:about="&fibo-fnd-bus-bg;CorporateGoal">
		<rdfs:subClassOf rdf:resource="&fibo-fnd-bus-bg;BusinessGoal"/>
		<rdfs:label xml:lang="en">corporate goal</rdfs:label>
		<skos:definition xml:lang="en">A business goal in the furtherance of the aims and profitability of a corporation.</skos:definition>
	</owl:Class>
	
	<owl:Class rdf:about="&fibo-fnd-bus-bg;FinancialWellbeing">
		<rdfs:subClassOf rdf:resource="&fibo-fnd-bus-bg;InvestmentGoal"/>
		<rdfs:label xml:lang="en">financial wellbeing</rdfs:label>
		<skos:definition xml:lang="en">The overall balance sheet and well being of the organisation.</skos:definition>
	</owl:Class>
	
	<owl:Class rdf:about="&fibo-fnd-bus-bg;InvestmentGoal">
		<rdfs:subClassOf rdf:resource="&fibo-fnd-bus-bg;BusinessGoal"/>
		<rdfs:label xml:lang="en">investment goal</rdfs:label>
		<skos:definition xml:lang="en">A goal for which is to be achieved by investments within an investment institution.</skos:definition>
	</owl:Class>
	
	<owl:Class rdf:about="&fibo-fnd-bus-bg;LendingGoal">
		<rdfs:subClassOf rdf:resource="&fibo-fnd-bus-bg;InvestmentGoal"/>
		<rdfs:label xml:lang="en">lending goal</rdfs:label>
		<skos:definition xml:lang="en">Reasons for extending loans and credit, i.e. the organisation has a goal to create capital growth by extending credit or making loans.</skos:definition>
	</owl:Class>
	
	<owl:Class rdf:about="&fibo-fnd-bus-bg;MarketInvestmentGoal">
		<rdfs:subClassOf rdf:resource="&fibo-fnd-bus-bg;InvestmentGoal"/>
		<rdfs:label xml:lang="en">market investment goal</rdfs:label>
		<skos:definition xml:lang="en">A business goal driving investment activities as distinct from day to day commercial trading activities.</skos:definition>
	</owl:Class>
	
	<owl:Class rdf:about="&fibo-fnd-bus-bg;ProjectGoal">
		<rdfs:subClassOf rdf:resource="&fibo-fnd-gao-gl;Goal"/>
		<rdfs:label xml:lang="en">project goal</rdfs:label>
		<skos:definition xml:lang="en">Some stated goal of a project as set out in the project planning documentation.</skos:definition>
		<fibo-fnd-utl-av:explanatoryNote xml:lang="en">Project risks are framed in terms of their impact on stated project goals. Examples including meeting deadlines, meeting cost projections, and so on.</fibo-fnd-utl-av:explanatoryNote>
	</owl:Class>
	
	<owl:Class rdf:about="&fibo-fnd-bus-bg;Reputation">
		<rdfs:subClassOf rdf:resource="&fibo-fnd-bus-bg;BusinessGoal"/>
		<rdfs:label xml:lang="en">reputation</rdfs:label>
		<skos:definition xml:lang="en">The goal of a business to maintain or enhance its reputation.</skos:definition>
	</owl:Class>
	
	<owl:Class rdf:about="&fibo-fnd-bus-bg;TransactionProcessingGoal">
		<rdfs:subClassOf rdf:resource="&fibo-fnd-bus-bg;InvestmentGoal"/>
		<rdfs:label xml:lang="en">transaction processing goal</rdfs:label>
		<skos:definition xml:lang="en">The goal of processing transactions in which the organization is engaged, without error and within the stated time constraints.</skos:definition>
	</owl:Class>

</rdf:RDF>