<?xml version="1.0" encoding="UTF-8"?>
<!DOCTYPE rdf:RDF [
	<!ENTITY dct "http://purl.org/dc/terms/">
	<!ENTITY fibo-be-le-fbo "https://spec.edmcouncil.org/fibo/BE/LegalEntities/FormalBusinessOrganizations/">
	<!ENTITY fibo-be-le-lei "https://spec.edmcouncil.org/fibo/BE/LegalEntities/LEIEntities/">
	<!ENTITY fibo-be-le-lp "https://spec.edmcouncil.org/fibo/BE/LegalEntities/LegalPersons/">
	<!ENTITY fibo-be-oac-opty "https://spec.edmcouncil.org/fibo/BE/OwnershipAndControl/OwnershipParties/">
	<!ENTITY fibo-fbc-dae-dbt "https://spec.edmcouncil.org/fibo/FBC/DebtAndEquities/Debt/">
	<!ENTITY fibo-fbc-dae-gty "https://spec.edmcouncil.org/fibo/FBC/DebtAndEquities/Guaranty/">
	<!ENTITY fibo-fbc-fct-rga "https://spec.edmcouncil.org/fibo/FBC/FunctionalEntities/RegulatoryAgencies/">
	<!ENTITY fibo-fbc-fi-fi "https://spec.edmcouncil.org/fibo/FBC/FinancialInstruments/FinancialInstruments/">
	<!ENTITY fibo-fbc-pas-caa "https://spec.edmcouncil.org/fibo/FBC/ProductsAndServices/ClientsAndAccounts/">
	<!ENTITY fibo-fbc-pas-fpas "https://spec.edmcouncil.org/fibo/FBC/ProductsAndServices/FinancialProductsAndServices/">
	<!ENTITY fibo-fnd-aap-agt "https://spec.edmcouncil.org/fibo/FND/AgentsAndPeople/Agents/">
	<!ENTITY fibo-fnd-aap-ppl "https://spec.edmcouncil.org/fibo/FND/AgentsAndPeople/People/">
	<!ENTITY fibo-fnd-acc-cur "https://spec.edmcouncil.org/fibo/FND/Accounting/CurrencyAmount/">
	<!ENTITY fibo-fnd-agr-agr "https://spec.edmcouncil.org/fibo/FND/Agreements/Agreements/">
	<!ENTITY fibo-fnd-agr-ctr "https://spec.edmcouncil.org/fibo/FND/Agreements/Contracts/">
	<!ENTITY fibo-fnd-arr-arr "https://spec.edmcouncil.org/fibo/FND/Arrangements/Arrangements/">
	<!ENTITY fibo-fnd-arr-cls "https://spec.edmcouncil.org/fibo/FND/Arrangements/ClassificationSchemes/">
	<!ENTITY fibo-fnd-arr-doc "https://spec.edmcouncil.org/fibo/FND/Arrangements/Documents/">
	<!ENTITY fibo-fnd-arr-id "https://spec.edmcouncil.org/fibo/FND/Arrangements/IdentifiersAndIndices/">
	<!ENTITY fibo-fnd-dt-fd "https://spec.edmcouncil.org/fibo/FND/DatesAndTimes/FinancialDates/">
	<!ENTITY fibo-fnd-dt-oc "https://spec.edmcouncil.org/fibo/FND/DatesAndTimes/Occurrences/">
	<!ENTITY fibo-fnd-oac-own "https://spec.edmcouncil.org/fibo/FND/OwnershipAndControl/Ownership/">
	<!ENTITY fibo-fnd-org-fm "https://spec.edmcouncil.org/fibo/FND/Organizations/FormalOrganizations/">
	<!ENTITY fibo-fnd-org-org "https://spec.edmcouncil.org/fibo/FND/Organizations/Organizations/">
	<!ENTITY fibo-fnd-pas-pas "https://spec.edmcouncil.org/fibo/FND/ProductsAndServices/ProductsAndServices/">
	<!ENTITY fibo-fnd-plc-adr "https://spec.edmcouncil.org/fibo/FND/Places/Addresses/">
	<!ENTITY fibo-fnd-plc-cr "https://spec.edmcouncil.org/fibo/FND/Places/CountryRepresentation/">
	<!ENTITY fibo-fnd-plc-cty "https://spec.edmcouncil.org/fibo/FND/Places/Countries/">
	<!ENTITY fibo-fnd-plc-loc "https://spec.edmcouncil.org/fibo/FND/Places/Locations/">
	<!ENTITY fibo-fnd-pty-pty "https://spec.edmcouncil.org/fibo/FND/Parties/Parties/">
	<!ENTITY fibo-fnd-qt-qtu "https://spec.edmcouncil.org/fibo/FND/Quantities/QuantitiesAndUnits/">
	<!ENTITY fibo-fnd-rel-rel "https://spec.edmcouncil.org/fibo/FND/Relations/Relations/">
	<!ENTITY fibo-fnd-utl-alx "https://spec.edmcouncil.org/fibo/FND/Utilities/Analytics/">
	<!ENTITY fibo-fnd-utl-av "https://spec.edmcouncil.org/fibo/FND/Utilities/AnnotationVocabulary/">
	<!ENTITY fibo-fnd-utl-bt "https://spec.edmcouncil.org/fibo/FND/Utilities/BusinessFacingTypes/">
	<!ENTITY fibo-fnd-utl-val "https://spec.edmcouncil.org/fibo/FND/Utilities/Values/">
	<!ENTITY fibo-ln-ln-ln "https://spec.edmcouncil.org/fibo/LOAN/LoanContracts/LoanCore/">
	<!ENTITY fibo-ln-ln-up "https://spec.edmcouncil.org/fibo/LOAN/LoanContracts/LoanUpperTemp/">
	<!ENTITY owl "http://www.w3.org/2002/07/owl#">
	<!ENTITY rdf "http://www.w3.org/1999/02/22-rdf-syntax-ns#">
	<!ENTITY rdfs "http://www.w3.org/2000/01/rdf-schema#">
	<!ENTITY skos "http://www.w3.org/2004/02/skos/core#">
	<!ENTITY sm "http://www.omg.org/techprocess/ab/SpecificationMetadata/">
	<!ENTITY xs "http://www.w3.org/2001/XMLSchema#">
]>
<rdf:RDF xml:base="https://spec.edmcouncil.org/fibo/LOAN/LoanContracts/LoanCore/"
	xmlns:dct="http://purl.org/dc/terms/"
	xmlns:fibo-be-le-fbo="https://spec.edmcouncil.org/fibo/BE/LegalEntities/FormalBusinessOrganizations/"
	xmlns:fibo-be-le-lei="https://spec.edmcouncil.org/fibo/BE/LegalEntities/LEIEntities/"
	xmlns:fibo-be-le-lp="https://spec.edmcouncil.org/fibo/BE/LegalEntities/LegalPersons/"
	xmlns:fibo-be-oac-opty="https://spec.edmcouncil.org/fibo/BE/OwnershipAndControl/OwnershipParties/"
	xmlns:fibo-fbc-dae-dbt="https://spec.edmcouncil.org/fibo/FBC/DebtAndEquities/Debt/"
	xmlns:fibo-fbc-dae-gty="https://spec.edmcouncil.org/fibo/FBC/DebtAndEquities/Guaranty/"
	xmlns:fibo-fbc-fct-rga="https://spec.edmcouncil.org/fibo/FBC/FunctionalEntities/RegulatoryAgencies/"
	xmlns:fibo-fbc-fi-fi="https://spec.edmcouncil.org/fibo/FBC/FinancialInstruments/FinancialInstruments/"
	xmlns:fibo-fbc-pas-caa="https://spec.edmcouncil.org/fibo/FBC/ProductsAndServices/ClientsAndAccounts/"
	xmlns:fibo-fbc-pas-fpas="https://spec.edmcouncil.org/fibo/FBC/ProductsAndServices/FinancialProductsAndServices/"
	xmlns:fibo-fnd-aap-agt="https://spec.edmcouncil.org/fibo/FND/AgentsAndPeople/Agents/"
	xmlns:fibo-fnd-aap-ppl="https://spec.edmcouncil.org/fibo/FND/AgentsAndPeople/People/"
	xmlns:fibo-fnd-acc-cur="https://spec.edmcouncil.org/fibo/FND/Accounting/CurrencyAmount/"
	xmlns:fibo-fnd-agr-agr="https://spec.edmcouncil.org/fibo/FND/Agreements/Agreements/"
	xmlns:fibo-fnd-agr-ctr="https://spec.edmcouncil.org/fibo/FND/Agreements/Contracts/"
	xmlns:fibo-fnd-arr-arr="https://spec.edmcouncil.org/fibo/FND/Arrangements/Arrangements/"
	xmlns:fibo-fnd-arr-cls="https://spec.edmcouncil.org/fibo/FND/Arrangements/ClassificationSchemes/"
	xmlns:fibo-fnd-arr-doc="https://spec.edmcouncil.org/fibo/FND/Arrangements/Documents/"
	xmlns:fibo-fnd-arr-id="https://spec.edmcouncil.org/fibo/FND/Arrangements/IdentifiersAndIndices/"
	xmlns:fibo-fnd-dt-fd="https://spec.edmcouncil.org/fibo/FND/DatesAndTimes/FinancialDates/"
	xmlns:fibo-fnd-dt-oc="https://spec.edmcouncil.org/fibo/FND/DatesAndTimes/Occurrences/"
	xmlns:fibo-fnd-oac-own="https://spec.edmcouncil.org/fibo/FND/OwnershipAndControl/Ownership/"
	xmlns:fibo-fnd-org-fm="https://spec.edmcouncil.org/fibo/FND/Organizations/FormalOrganizations/"
	xmlns:fibo-fnd-org-org="https://spec.edmcouncil.org/fibo/FND/Organizations/Organizations/"
	xmlns:fibo-fnd-pas-pas="https://spec.edmcouncil.org/fibo/FND/ProductsAndServices/ProductsAndServices/"
	xmlns:fibo-fnd-plc-adr="https://spec.edmcouncil.org/fibo/FND/Places/Addresses/"
	xmlns:fibo-fnd-plc-cr="https://spec.edmcouncil.org/fibo/FND/Places/CountryRepresentation/"
	xmlns:fibo-fnd-plc-cty="https://spec.edmcouncil.org/fibo/FND/Places/Countries/"
	xmlns:fibo-fnd-plc-loc="https://spec.edmcouncil.org/fibo/FND/Places/Locations/"
	xmlns:fibo-fnd-pty-pty="https://spec.edmcouncil.org/fibo/FND/Parties/Parties/"
	xmlns:fibo-fnd-qt-qtu="https://spec.edmcouncil.org/fibo/FND/Quantities/QuantitiesAndUnits/"
	xmlns:fibo-fnd-rel-rel="https://spec.edmcouncil.org/fibo/FND/Relations/Relations/"
	xmlns:fibo-fnd-utl-alx="https://spec.edmcouncil.org/fibo/FND/Utilities/Analytics/"
	xmlns:fibo-fnd-utl-av="https://spec.edmcouncil.org/fibo/FND/Utilities/AnnotationVocabulary/"
	xmlns:fibo-fnd-utl-bt="https://spec.edmcouncil.org/fibo/FND/Utilities/BusinessFacingTypes/"
	xmlns:fibo-fnd-utl-val="https://spec.edmcouncil.org/fibo/FND/Utilities/Values/"
	xmlns:fibo-ln-ln-ln="https://spec.edmcouncil.org/fibo/LOAN/LoanContracts/LoanCore/"
	xmlns:fibo-ln-ln-up="https://spec.edmcouncil.org/fibo/LOAN/LoanContracts/LoanUpperTemp/"
	xmlns:owl="http://www.w3.org/2002/07/owl#"
	xmlns:rdf="http://www.w3.org/1999/02/22-rdf-syntax-ns#"
	xmlns:rdfs="http://www.w3.org/2000/01/rdf-schema#"
	xmlns:skos="http://www.w3.org/2004/02/skos/core#"
	xmlns:sm="http://www.omg.org/techprocess/ab/SpecificationMetadata/"
	xmlns:xs="http://www.w3.org/2001/XMLSchema#">
	
	<owl:Ontology rdf:about="https://spec.edmcouncil.org/fibo/LOAN/LoanContracts/LoanCore/">
		<rdfs:comment></rdfs:comment>
		<rdfs:comment>loanCore</rdfs:comment>
		<owl:imports rdf:resource="http://www.w3.org/2004/02/skos/core"/>
		<owl:imports rdf:resource="https://spec.edmcouncil.org/fibo/BE/LegalEntities/LEIEntities/"/>
		<owl:imports rdf:resource="https://spec.edmcouncil.org/fibo/FBC/DebtAndEquities/Debt/"/>
		<owl:imports rdf:resource="https://spec.edmcouncil.org/fibo/FBC/DebtAndEquities/Guaranty/"/>
		<owl:imports rdf:resource="https://spec.edmcouncil.org/fibo/FBC/FinancialInstruments/FinancialInstruments/"/>
		<owl:imports rdf:resource="https://spec.edmcouncil.org/fibo/FBC/ProductsAndServices/ClientsAndAccounts/"/>
		<owl:imports rdf:resource="https://spec.edmcouncil.org/fibo/FBC/ProductsAndServices/FinancialProductsAndServices/"/>
		<owl:imports rdf:resource="https://spec.edmcouncil.org/fibo/FND/Accounting/CurrencyAmount/"/>
		<owl:imports rdf:resource="https://spec.edmcouncil.org/fibo/FND/AgentsAndPeople/Agents/"/>
		<owl:imports rdf:resource="https://spec.edmcouncil.org/fibo/FND/AgentsAndPeople/People/"/>
		<owl:imports rdf:resource="https://spec.edmcouncil.org/fibo/FND/Agreements/Agreements/"/>
		<owl:imports rdf:resource="https://spec.edmcouncil.org/fibo/FND/Agreements/Contracts/"/>
		<owl:imports rdf:resource="https://spec.edmcouncil.org/fibo/FND/Arrangements/Arrangements/"/>
		<owl:imports rdf:resource="https://spec.edmcouncil.org/fibo/FND/Arrangements/ClassificationSchemes/"/>
		<owl:imports rdf:resource="https://spec.edmcouncil.org/fibo/FND/Arrangements/Documents/"/>
		<owl:imports rdf:resource="https://spec.edmcouncil.org/fibo/FND/Arrangements/IdentifiersAndIndices/"/>
		<owl:imports rdf:resource="https://spec.edmcouncil.org/fibo/FND/DatesAndTimes/FinancialDates/"/>
		<owl:imports rdf:resource="https://spec.edmcouncil.org/fibo/FND/DatesAndTimes/Occurrences/"/>
		<owl:imports rdf:resource="https://spec.edmcouncil.org/fibo/FND/Organizations/FormalOrganizations/"/>
		<owl:imports rdf:resource="https://spec.edmcouncil.org/fibo/FND/OwnershipAndControl/Ownership/"/>
		<owl:imports rdf:resource="https://spec.edmcouncil.org/fibo/FND/Parties/Parties/"/>
		<owl:imports rdf:resource="https://spec.edmcouncil.org/fibo/FND/Places/Addresses/"/>
		<owl:imports rdf:resource="https://spec.edmcouncil.org/fibo/FND/Places/Locations/"/>
		<owl:imports rdf:resource="https://spec.edmcouncil.org/fibo/FND/Quantities/QuantitiesAndUnits/"/>
		<owl:imports rdf:resource="https://spec.edmcouncil.org/fibo/FND/Relations/Relations/"/>
		<owl:imports rdf:resource="https://spec.edmcouncil.org/fibo/FND/Utilities/AnnotationVocabulary/"/>
		<owl:imports rdf:resource="https://spec.edmcouncil.org/fibo/FND/Utilities/BusinessFacingTypes/"/>
		<owl:imports rdf:resource="https://spec.edmcouncil.org/fibo/LOAN/LoanContracts/LoanUpperTemp/"/>
		<owl:versionInfo>Created with e6Tools Graphical OWL Editor from D:\SEMANTIC-ARTS\NAS\ClientsAndPartners\EDM Council\fibo ontologies\LoanOntology\loans.vsdx Page:loanCore</owl:versionInfo>
	</owl:Ontology>
	
	<owl:ObjectProperty rdf:about="&fibo-fnd-acc-cur;hasNotionalAmount">
		<rdfs:subPropertyOf rdf:resource="&fibo-ln-ln-up;cur-hasAmount"/>
	</owl:ObjectProperty>
	
	<fibo-fnd-pty-pty:IndependentParty rdf:about="&fibo-fnd-pty-pty;_FHA">
		<rdf:type rdf:resource="&owl;Thing"/>
		<rdfs:label>Federal Housing Authority</rdfs:label>
	</fibo-fnd-pty-pty:IndependentParty>
	
	<fibo-fnd-pty-pty:IndependentParty rdf:about="&fibo-fnd-pty-pty;_FannieMae">
		<rdf:type rdf:resource="&owl;Thing"/>
		<rdfs:label>Fannie Mae</rdfs:label>
	</fibo-fnd-pty-pty:IndependentParty>
	
	<fibo-fnd-pty-pty:IndependentParty rdf:about="&fibo-fnd-pty-pty;_FreddieMac">
		<rdf:type rdf:resource="&owl;Thing"/>
		<rdfs:label>Freddie Mac</rdfs:label>
	</fibo-fnd-pty-pty:IndependentParty>
	
	<fibo-fnd-pty-pty:IndependentParty rdf:about="&fibo-fnd-pty-pty;_USDA">
		<rdf:type rdf:resource="&owl;Thing"/>
		<rdfs:label>US Dept. of Agriculture</rdfs:label>
	</fibo-fnd-pty-pty:IndependentParty>
	
	<fibo-fnd-pty-pty:IndependentParty rdf:about="&fibo-fnd-pty-pty;_VA">
		<rdf:type rdf:resource="&owl;Thing"/>
		<rdfs:label>Veterans Administration</rdfs:label>
	</fibo-fnd-pty-pty:IndependentParty>
	
	<owl:Class rdf:about="&fibo-fnd-plc-loc;RealEstate">
		<rdfs:subClassOf>
			<owl:Restriction>
				<owl:onProperty rdf:resource="&fibo-ln-ln-up;cur-hasEstimatedValue"/>
				<owl:onClass rdf:resource="&fibo-fnd-acc-cur;MonetaryAmount"/>
				<owl:minQualifiedCardinality rdf:datatype="&xs;nonNegativeInteger">0</owl:minQualifiedCardinality>
			</owl:Restriction>
		</rdfs:subClassOf>
		<rdfs:subClassOf>
			<owl:Restriction>
				<owl:onProperty rdf:resource="&fibo-fnd-rel-rel;has"/>
				<owl:onClass rdf:resource="&fibo-fnd-plc-adr;PostalAddress"/>
				<owl:minQualifiedCardinality rdf:datatype="&xs;nonNegativeInteger">0</owl:minQualifiedCardinality>
			</owl:Restriction>
		</rdfs:subClassOf>
		<rdfs:subClassOf>
			<owl:Restriction>
				<owl:onProperty rdf:resource="&fibo-fnd-rel-rel;has"/>
				<owl:onClass rdf:resource="&fibo-ln-ln-ln;RealPropertyAppraisal"/>
				<owl:minQualifiedCardinality rdf:datatype="&xs;nonNegativeInteger">0</owl:minQualifiedCardinality>
			</owl:Restriction>
		</rdfs:subClassOf>
		<rdfs:subClassOf>
			<owl:Restriction>
				<owl:onProperty rdf:resource="&fibo-fnd-rel-rel;isClassifiedBy"/>
				<owl:someValuesFrom rdf:resource="&fibo-ln-ln-ln;ConstructionType"/>
			</owl:Restriction>
		</rdfs:subClassOf>
		<rdfs:subClassOf>
			<owl:Restriction>
				<owl:onProperty rdf:resource="&fibo-fnd-rel-rel;isClassifiedBy"/>
				<owl:someValuesFrom rdf:resource="&fibo-ln-ln-ln;DwellingCapacity"/>
			</owl:Restriction>
		</rdfs:subClassOf>
	</owl:Class>
	
	<owl:Class rdf:about="&fibo-ln-ln-ln;AmortizationSchedule">
		<rdfs:subClassOf rdf:resource="&fibo-fnd-arr-arr;Collection"/>
		<skos:definition>A schedule which specifies changes in the scheduled balance of loan principal over time.</skos:definition>
		<skos:editorialNote>If needed, we can extend this to include the idea of an AmortizationScheduledPayment which includes interest and principal and many of which comprise an AmortizationSchedule</skos:editorialNote>
		<fibo-fnd-utl-av:explanatoryNote>For simplicity, this definition assums that &apos;month n&apos; &apos; on an AmortizationSchedule corresoponds to a CalculatedDate.</fibo-fnd-utl-av:explanatoryNote>
	</owl:Class>
	
	<owl:Class rdf:about="&fibo-ln-ln-ln;CashOutStatus">
		<rdfs:subClassOf rdf:resource="&fibo-fnd-arr-cls;Classifier"/>
		<skos:definition>A category indicating the extent to which funds are released to the borrower on a new loan origination that is  refinancing an existing loan. Subject to lender and/or investor policy(s).</skos:definition>
	</owl:Class>
	
	<owl:Class rdf:about="&fibo-ln-ln-ln;ClosedEndLoanContract">
		<rdfs:subClassOf rdf:resource="&fibo-fbc-fi-fi;DebtInstrument"/>
		<rdfs:subClassOf rdf:resource="&fibo-ln-ln-ln;LoanContract"/>
		<rdfs:subClassOf>
			<owl:Restriction>
				<owl:onProperty rdf:resource="&fibo-ln-ln-ln;hasNoteAmount"/>
				<owl:someValuesFrom rdf:resource="&fibo-fnd-acc-cur;MonetaryAmount"/>
			</owl:Restriction>
		</rdfs:subClassOf>
		<skos:definition>A LoanContract that has an amount borrowed for a fixed amount of time, and is not considered open ended.</skos:definition>
		<fibo-fnd-utl-av:adaptedFrom>2015 Revised HMDA regulation</fibo-fnd-utl-av:adaptedFrom>
	</owl:Class>
	
	<owl:Class rdf:about="&fibo-ln-ln-ln;ConstructionType">
		<rdfs:subClassOf rdf:resource="&fibo-fnd-arr-cls;Classifier"/>
		<skos:definition>A particular kind of construction</skos:definition>
	</owl:Class>
	
	<owl:Class rdf:about="&fibo-ln-ln-ln;CreditEvaluationProduct">
		<rdfs:subClassOf rdf:resource="&fibo-ln-ln-up;FND-InformationProduct"/>
		<skos:definition>A specific kind of credit evaluation.</skos:definition>
	</owl:Class>
	
	<owl:Class rdf:about="&fibo-ln-ln-ln;CreditInquiry">
		<rdfs:subClassOf>
			<owl:Class>
				<owl:intersectionOf rdf:parseType="Collection">
					<rdf:Description rdf:about="&fibo-ln-ln-up;fnd-Request">
					</rdf:Description>
					<owl:Restriction>
						<owl:onProperty rdf:resource="&fibo-fnd-rel-rel;isClassifiedBy"/>
						<owl:someValuesFrom rdf:resource="&fibo-ln-ln-ln;CreditInquiryType"/>
					</owl:Restriction>
				</owl:intersectionOf>
			</owl:Class>
		</rdfs:subClassOf>
		<rdfs:subClassOf>
			<owl:Restriction>
				<owl:onProperty rdf:resource="&fibo-ln-ln-ln;hasPartyBeingChecked"/>
				<owl:someValuesFrom rdf:resource="&fibo-fnd-pty-pty;IndependentParty"/>
			</owl:Restriction>
		</rdfs:subClassOf>
		<rdfs:subClassOf>
			<owl:Restriction>
				<owl:onProperty rdf:resource="&fibo-ln-ln-up;rel-from"/>
				<owl:someValuesFrom rdf:resource="&fibo-fnd-pty-pty;IndependentParty"/>
			</owl:Restriction>
		</rdfs:subClassOf>
		<rdfs:subClassOf>
			<owl:Restriction>
				<owl:onProperty rdf:resource="&fibo-ln-ln-up;rel-to"/>
				<owl:someValuesFrom rdf:resource="&fibo-ln-ln-ln;CreditRepository_I"/>
			</owl:Restriction>
		</rdfs:subClassOf>
		<skos:definition>A request from a lender to a credit repository to obtain information regarding a prospective borrower&apos;s creditworthiness.</skos:definition>
	</owl:Class>
	
	<owl:Class rdf:about="&fibo-ln-ln-ln;CreditInquiryType">
		<rdfs:subClassOf rdf:resource="&fibo-fnd-arr-cls;Classifier"/>
		<skos:definition>A category indicating whether a credit inquiry is a result of a borrower&apos;s direct authorization or by some indirect means.</skos:definition>
	</owl:Class>
	
	<owl:Class rdf:about="&fibo-ln-ln-ln;CreditMessage">
		<rdfs:subClassOf>
			<owl:Class>
				<owl:intersectionOf rdf:parseType="Collection">
					<rdf:Description rdf:about="&fibo-fnd-utl-val;TextValue">
					</rdf:Description>
					<owl:Restriction>
						<owl:onProperty rdf:resource="&fibo-fnd-rel-rel;isClassifiedBy"/>
						<owl:someValuesFrom rdf:resource="&fibo-ln-ln-ln;CreditMessageType"/>
					</owl:Restriction>
				</owl:intersectionOf>
			</owl:Class>
		</rdfs:subClassOf>
		<skos:definition>A textual annotation on a credit report to notify a reviewer of special or exceptional information.</skos:definition>
	</owl:Class>
	
	<owl:Class rdf:about="&fibo-ln-ln-ln;CreditMessageType">
		<rdfs:subClassOf rdf:resource="&fibo-fnd-arr-cls;Classifier"/>
		<skos:definition>A specific kind of credit message.</skos:definition>
	</owl:Class>
	
	<owl:Class rdf:about="&fibo-ln-ln-ln;CreditReport">
		<rdfs:subClassOf rdf:resource="&fibo-ln-ln-up;Report"/>
		<rdfs:subClassOf>
			<owl:Restriction>
				<owl:onProperty rdf:resource="&fibo-fnd-rel-rel;comprises"/>
				<owl:onClass rdf:resource="&fibo-ln-ln-ln;CreditInquiry"/>
				<owl:minQualifiedCardinality rdf:datatype="&xs;nonNegativeInteger">0</owl:minQualifiedCardinality>
			</owl:Restriction>
		</rdfs:subClassOf>
		<rdfs:subClassOf>
			<owl:Restriction>
				<owl:onProperty rdf:resource="&fibo-fnd-rel-rel;comprises"/>
				<owl:onClass rdf:resource="&fibo-ln-ln-ln;CreditScore"/>
				<owl:minQualifiedCardinality rdf:datatype="&xs;nonNegativeInteger">0</owl:minQualifiedCardinality>
			</owl:Restriction>
		</rdfs:subClassOf>
		<rdfs:subClassOf>
			<owl:Restriction>
				<owl:onProperty rdf:resource="&fibo-fnd-rel-rel;comprises"/>
				<owl:onClass rdf:resource="&fibo-ln-ln-ln;CreditTradeLine"/>
				<owl:minQualifiedCardinality rdf:datatype="&xs;nonNegativeInteger">0</owl:minQualifiedCardinality>
			</owl:Restriction>
		</rdfs:subClassOf>
		<rdfs:subClassOf>
			<owl:Restriction>
				<owl:onProperty rdf:resource="&fibo-fnd-rel-rel;comprises"/>
				<owl:onClass rdf:resource="&fibo-ln-ln-ln;PublicRecord"/>
				<owl:minQualifiedCardinality rdf:datatype="&xs;nonNegativeInteger">0</owl:minQualifiedCardinality>
			</owl:Restriction>
		</rdfs:subClassOf>
		<rdfs:subClassOf>
			<owl:Restriction>
				<owl:onProperty rdf:resource="&fibo-fnd-aap-agt;isIdentifiedBy"/>
				<owl:someValuesFrom rdf:resource="&fibo-fnd-arr-id;Identifier"/>
			</owl:Restriction>
		</rdfs:subClassOf>
		<rdfs:subClassOf>
			<owl:Restriction>
				<owl:onProperty rdf:resource="&fibo-fnd-rel-rel;comprises"/>
				<owl:someValuesFrom rdf:resource="&fibo-ln-ln-ln;CreditMessage"/>
			</owl:Restriction>
		</rdfs:subClassOf>
		<rdfs:subClassOf>
			<owl:Restriction>
				<owl:onProperty rdf:resource="&fibo-fnd-rel-rel;isClassifiedBy"/>
				<owl:someValuesFrom rdf:resource="&fibo-ln-ln-ln;CreditReportCategory"/>
			</owl:Restriction>
		</rdfs:subClassOf>
		<rdfs:subClassOf>
			<owl:Restriction>
				<owl:onProperty rdf:resource="&fibo-ln-ln-ln;hasCoveragePeriod"/>
				<owl:someValuesFrom rdf:resource="&fibo-fnd-dt-fd;DatePeriod"/>
			</owl:Restriction>
		</rdfs:subClassOf>
		<rdfs:subClassOf>
			<owl:Restriction>
				<owl:onProperty rdf:resource="&fibo-ln-ln-ln;hasPartyBeingChecked"/>
				<owl:someValuesFrom rdf:resource="&fibo-fnd-pty-pty;IndependentParty"/>
			</owl:Restriction>
		</rdfs:subClassOf>
		<rdfs:subClassOf>
			<owl:Restriction>
				<owl:onProperty rdf:resource="&fibo-ln-ln-up;asOfDate"/>
				<owl:someValuesFrom rdf:resource="&fibo-fnd-dt-fd;Date"/>
			</owl:Restriction>
		</rdfs:subClassOf>
		<rdfs:subClassOf>
			<owl:Restriction>
				<owl:onProperty rdf:resource="&fibo-ln-ln-up;dataSourcedFrom"/>
				<owl:someValuesFrom rdf:resource="&fibo-ln-ln-ln;CreditRepository_I"/>
			</owl:Restriction>
		</rdfs:subClassOf>
		<rdfs:subClassOf>
			<owl:Restriction>
				<owl:onProperty rdf:resource="&fibo-ln-ln-up;instantiates"/>
				<owl:someValuesFrom rdf:resource="&fibo-ln-ln-ln;CreditReportProduct"/>
			</owl:Restriction>
		</rdfs:subClassOf>
		<rdfs:subClassOf>
			<owl:Restriction>
				<owl:onProperty rdf:resource="&fibo-ln-ln-up;rel-isProducedBy_I"/>
				<owl:someValuesFrom rdf:resource="&fibo-ln-ln-ln;CreditReportingAgency_I"/>
			</owl:Restriction>
		</rdfs:subClassOf>
		<skos:definition>A report describing the credit worthiness and related credit attributes of a borrower. This is typically provided by a credit reporting agency but could be produced by an internal proprietary model as well.</skos:definition>
	</owl:Class>
	
	<owl:Class rdf:about="&fibo-ln-ln-ln;CreditReportCategory">
		<rdfs:subClassOf rdf:resource="&fibo-fnd-arr-cls;Classifier"/>
		<skos:definition>A specific kind of credit report, often available from multiple vendors.</skos:definition>
	</owl:Class>
	
	<owl:Class rdf:about="&fibo-ln-ln-ln;CreditReportProduct">
		<rdfs:subClassOf rdf:resource="&fibo-ln-ln-ln;CreditEvaluationProduct"/>
		<skos:definition>A specifically branded credit report offered in the market place.</skos:definition>
	</owl:Class>
	
	<owl:Class rdf:about="&fibo-ln-ln-ln;CreditReportRequest">
		<rdfs:subClassOf rdf:resource="&fibo-ln-ln-up;fnd-Request"/>
		<rdfs:subClassOf>
			<owl:Restriction>
				<owl:onProperty rdf:resource="&fibo-ln-ln-ln;hasPartyBeingChecked"/>
				<owl:someValuesFrom rdf:resource="&fibo-fnd-pty-pty;IndependentParty"/>
			</owl:Restriction>
		</rdfs:subClassOf>
		<rdfs:subClassOf>
			<owl:Restriction>
				<owl:onProperty rdf:resource="&fibo-ln-ln-up;fnd-thingRequested"/>
				<owl:someValuesFrom rdf:resource="&fibo-ln-ln-ln;CreditReportProduct"/>
			</owl:Restriction>
		</rdfs:subClassOf>
		<rdfs:subClassOf>
			<owl:Restriction>
				<owl:onProperty rdf:resource="&fibo-ln-ln-up;rel-from"/>
				<owl:someValuesFrom rdf:resource="&fibo-fnd-pty-pty;IndependentParty"/>
			</owl:Restriction>
		</rdfs:subClassOf>
		<rdfs:subClassOf>
			<owl:Restriction>
				<owl:onProperty rdf:resource="&fibo-ln-ln-up;rel-to"/>
				<owl:someValuesFrom>
					<owl:Class>
						<owl:unionOf rdf:parseType="Collection">
							<rdf:Description rdf:about="&fibo-ln-ln-ln;CreditReportingAgency_I">
							</rdf:Description>
							<rdf:Description rdf:about="&fibo-ln-ln-ln;CreditRepository_I">
							</rdf:Description>
						</owl:unionOf>
					</owl:Class>
				</owl:someValuesFrom>
			</owl:Restriction>
		</rdfs:subClassOf>
		<skos:definition>The act of requesting a credit report from a credit reporting provider.</skos:definition>
	</owl:Class>
	
	<owl:Class rdf:about="&fibo-ln-ln-ln;CreditReportResponse">
		<rdfs:subClassOf rdf:resource="&fibo-ln-ln-up;fnd-Response"/>
		<rdfs:subClassOf>
			<owl:Restriction>
				<owl:onProperty rdf:resource="&fibo-ln-ln-up;fnd-rel-isResponseTo"/>
				<owl:someValuesFrom rdf:resource="&fibo-ln-ln-ln;CreditReportRequest"/>
			</owl:Restriction>
		</rdfs:subClassOf>
		<rdfs:subClassOf>
			<owl:Restriction>
				<owl:onProperty rdf:resource="&fibo-ln-ln-up;rel-from"/>
				<owl:someValuesFrom rdf:resource="&fibo-fnd-aap-agt;AutonomousAgent"/>
			</owl:Restriction>
		</rdfs:subClassOf>
		<rdfs:subClassOf>
			<owl:Restriction>
				<owl:onProperty rdf:resource="&fibo-ln-ln-up;rel-to"/>
				<owl:someValuesFrom rdf:resource="&fibo-fnd-aap-agt;AutonomousAgent"/>
			</owl:Restriction>
		</rdfs:subClassOf>
		<skos:definition>The act of responding to a credit report request.</skos:definition>
	</owl:Class>
	
	<owl:Class rdf:about="&fibo-ln-ln-ln;CreditReportingAgency_I">
		<rdfs:subClassOf rdf:resource="&fibo-fnd-pty-pty;IndependentParty"/>
		<skos:definition>This is the independent party, not the party in role</skos:definition>
	</owl:Class>
	
	<owl:Class rdf:about="&fibo-ln-ln-ln;CreditRepository_I">
		<rdfs:subClassOf rdf:resource="&fibo-fnd-pty-pty;IndependentParty"/>
		<skos:definition>This is the independent party, not the party in role</skos:definition>
	</owl:Class>
	
	<owl:Class rdf:about="&fibo-ln-ln-ln;CreditRiskAssessment">
		<rdfs:subClassOf rdf:resource="&fibo-ln-ln-up;fnd-RiskAssesssment"/>
		<rdfs:subClassOf>
			<owl:Restriction>
				<owl:onProperty rdf:resource="&fibo-ln-ln-up;hasInput"/>
				<owl:someValuesFrom rdf:resource="&fibo-ln-ln-ln;CreditReport"/>
			</owl:Restriction>
		</rdfs:subClassOf>
		<rdfs:subClassOf>
			<owl:Restriction>
				<owl:onProperty rdf:resource="&fibo-ln-ln-up;hasInput"/>
				<owl:someValuesFrom rdf:resource="&fibo-ln-ln-ln;PreApprovalContract"/>
			</owl:Restriction>
		</rdfs:subClassOf>
		<rdfs:subClassOf>
			<owl:Restriction>
				<owl:onProperty rdf:resource="&fibo-ln-ln-up;hasInput"/>
				<owl:someValuesFrom rdf:resource="&fibo-ln-ln-ln;PreApprovalRequest"/>
			</owl:Restriction>
		</rdfs:subClassOf>
		<skos:definition>A kind of RiskAssessment that focuses on determining the likelihood of a potential borrower repaying a loan.</skos:definition>
	</owl:Class>
	
	<owl:Class rdf:about="&fibo-ln-ln-ln;CreditScore">
		<rdfs:subClassOf>
			<owl:Restriction>
				<owl:onProperty rdf:resource="&fibo-fnd-rel-rel;has"/>
				<owl:onClass rdf:resource="&fibo-ln-ln-ln;CreditScoreFactor"/>
				<owl:minQualifiedCardinality rdf:datatype="&xs;nonNegativeInteger">0</owl:minQualifiedCardinality>
			</owl:Restriction>
		</rdfs:subClassOf>
		<rdfs:subClassOf>
			<owl:Restriction>
				<owl:onProperty rdf:resource="&fibo-fnd-qt-qtu;isDerivedFrom"/>
				<owl:someValuesFrom rdf:resource="&fibo-ln-ln-ln;CreditScoreModel"/>
			</owl:Restriction>
		</rdfs:subClassOf>
		<owl:equivalentClass>
			<owl:Class>
				<owl:unionOf rdf:parseType="Collection">
					<rdf:Description rdf:about="&fibo-ln-ln-ln;CreditScoreNumber">
					</rdf:Description>
					<rdf:Description rdf:about="&fibo-ln-ln-ln;CreditScoreCategory">
					</rdf:Description>
				</owl:unionOf>
			</owl:Class>
		</owl:equivalentClass>
		<skos:definition>A quantitative measure or category that results from a credit evaluation model.</skos:definition>
	</owl:Class>
	
	<owl:Class rdf:about="&fibo-ln-ln-ln;CreditScoreCategory">
		<rdfs:subClassOf rdf:resource="&fibo-fnd-arr-cls;Classifier"/>
		<skos:definition>A CreditScore that is a qualitative measure.</skos:definition>
	</owl:Class>
	
	<owl:Class rdf:about="&fibo-ln-ln-ln;CreditScoreModel">
		<rdfs:subClassOf>
			<owl:Class>
				<owl:intersectionOf rdf:parseType="Collection">
					<rdf:Description rdf:about="&fibo-fnd-utl-alx;CalculationFormula">
					</rdf:Description>
					<owl:Restriction>
						<owl:onProperty rdf:resource="&fibo-fnd-rel-rel;isClassifiedBy"/>
						<owl:someValuesFrom rdf:resource="&fibo-ln-ln-ln;CreditScoreModelType"/>
					</owl:Restriction>
				</owl:intersectionOf>
			</owl:Class>
		</rdfs:subClassOf>
		<rdfs:subClassOf>
			<owl:Restriction>
				<owl:onProperty rdf:resource="&fibo-fnd-aap-agt;hasName"/>
				<owl:someValuesFrom rdf:resource="&xs;string"/>
			</owl:Restriction>
		</rdfs:subClassOf>
		<rdfs:subClassOf>
			<owl:Restriction>
				<owl:onProperty rdf:resource="&fibo-ln-ln-up;rel-hasVersion"/>
				<owl:someValuesFrom rdf:resource="&xs;string"/>
			</owl:Restriction>
		</rdfs:subClassOf>
		<skos:definition>An algorithm for computing the credit score of e.g. a credit applicant.</skos:definition>
	</owl:Class>
	
	<owl:Class rdf:about="&fibo-ln-ln-ln;CreditScoreModelType">
		<rdfs:subClassOf rdf:resource="&fibo-fnd-arr-cls;Classifier"/>
		<skos:definition>A family of credit scoring algorithms sharing common characteristics.</skos:definition>
	</owl:Class>
	
	<owl:Class rdf:about="&fibo-ln-ln-ln;CreditScoreNumber">
		<rdfs:subClassOf>
			<owl:Restriction>
				<owl:onProperty rdf:resource="&fibo-fnd-qt-qtu;hasNumericValue"/>
				<owl:someValuesFrom rdf:resource="&xs;decimal"/>
			</owl:Restriction>
		</rdfs:subClassOf>
		<skos:definition>A CreditScore that is a quantitative measure.</skos:definition>
	</owl:Class>
	
	<owl:Class rdf:about="&fibo-ln-ln-ln;CreditTradeLine">
		<rdfs:subClassOf>
			<owl:Restriction>
				<owl:onProperty rdf:resource="&fibo-fnd-qt-qtu;isDerivedFrom"/>
				<owl:someValuesFrom rdf:resource="&fibo-ln-ln-up;TransactionHistory"/>
			</owl:Restriction>
		</rdfs:subClassOf>
		<rdfs:subClassOf>
			<owl:Restriction>
				<owl:onProperty rdf:resource="&fibo-fnd-rel-rel;isPartOf"/>
				<owl:someValuesFrom rdf:resource="&fibo-ln-ln-ln;CreditReport"/>
			</owl:Restriction>
		</rdfs:subClassOf>
		<skos:definition>An information product derived from the transaction history of a credit account.</skos:definition>
	</owl:Class>
	
	<owl:Class rdf:about="&fibo-ln-ln-ln;DwellingCapacity">
		<rdfs:subClassOf rdf:resource="&fibo-fnd-arr-cls;Classifier"/>
		<skos:definition>A category indicating how many dwellings some property has.</skos:definition>
	</owl:Class>
	
	<owl:Class rdf:about="&fibo-ln-ln-ln;Ethnicity">
		<rdfs:subClassOf>
			<owl:Restriction>
				<owl:onProperty rdf:resource="&skos;broaderTransitive"/>
				<owl:someValuesFrom rdf:resource="&fibo-ln-ln-ln;Ethnicity"/>
			</owl:Restriction>
		</rdfs:subClassOf>
		<rdfs:subClassOf>
			<owl:Restriction>
				<owl:onProperty rdf:resource="&fibo-fnd-rel-rel;classifies"/>
				<owl:someValuesFrom rdf:resource="&fibo-fnd-aap-ppl;Person"/>
			</owl:Restriction>
		</rdfs:subClassOf>
		<skos:definition>A category based on a cultural factors, including nationality, regional culture, ancestry, and language</skos:definition>
	</owl:Class>
	
	<owl:Class rdf:about="&fibo-ln-ln-ln;IsPreApprovalRequested">
		<rdfs:subClassOf rdf:resource="&fibo-fnd-arr-cls;Classifier"/>
		<skos:definition>A category indicating whether a pre-approval has been requested, in conjunction with a loan application.</skos:definition>
	</owl:Class>
	
	<owl:Class rdf:about="&fibo-ln-ln-ln;LenderLienPosition">
		<rdfs:subClassOf rdf:resource="&fibo-fnd-arr-cls;Classifier"/>
		<skos:definition>Indicates whether the lender has the primary lien position</skos:definition>
	</owl:Class>
	
	<owl:Class rdf:about="&fibo-ln-ln-ln;LoanApplication">
		<rdfs:subClassOf rdf:resource="&fibo-ln-ln-up;Application"/>
		<skos:definition>A request of a potential borrower to a potential lender to borrow money.  It contains information used to decide whether to grant the loan.</skos:definition>
	</owl:Class>
	
	<owl:Class rdf:about="&fibo-ln-ln-ln;LoanContract">
		<rdfs:subClassOf rdf:resource="&fibo-fbc-dae-dbt;CreditAgreement"/>
		<rdfs:subClassOf rdf:resource="&fibo-fnd-agr-ctr;WrittenContract"/>
		<rdfs:subClassOf>
			<owl:Restriction>
				<owl:onProperty rdf:resource="&fibo-fnd-rel-rel;has"/>
				<owl:onClass rdf:resource="&fibo-fbc-dae-gty;Guaranty"/>
				<owl:minQualifiedCardinality rdf:datatype="&xs;nonNegativeInteger">0</owl:minQualifiedCardinality>
			</owl:Restriction>
		</rdfs:subClassOf>
		<rdfs:subClassOf>
			<owl:Restriction>
				<owl:onProperty rdf:resource="&fibo-ln-ln-up;rel-produces_I"/>
				<owl:onClass rdf:resource="&fibo-ln-ln-ln;ObligationToPay"/>
				<owl:minQualifiedCardinality rdf:datatype="&xs;nonNegativeInteger">0</owl:minQualifiedCardinality>
			</owl:Restriction>
		</rdfs:subClassOf>
		<rdfs:subClassOf>
			<owl:Restriction>
				<owl:onProperty rdf:resource="&fibo-ln-ln-up;rel-produces_I"/>
				<owl:onClass rdf:resource="&fibo-ln-ln-ln;ObligationToRepay"/>
				<owl:minQualifiedCardinality rdf:datatype="&xs;nonNegativeInteger">0</owl:minQualifiedCardinality>
			</owl:Restriction>
		</rdfs:subClassOf>
		<rdfs:subClassOf>
			<owl:Restriction>
				<owl:onProperty rdf:resource="&fibo-fnd-rel-rel;comprises"/>
				<owl:onClass rdf:resource="&fibo-ln-ln-ln;SecurityAgreement"/>
				<owl:minQualifiedCardinality rdf:datatype="&xs;nonNegativeInteger">0</owl:minQualifiedCardinality>
			</owl:Restriction>
		</rdfs:subClassOf>
		<rdfs:subClassOf>
			<owl:Restriction>
				<owl:onProperty rdf:resource="&fibo-fnd-aap-agt;isIdentifiedBy"/>
				<owl:onClass rdf:resource="&fibo-ln-ln-ln;UniversalLoanIdentifier"/>
				<owl:minQualifiedCardinality rdf:datatype="&xs;nonNegativeInteger">0</owl:minQualifiedCardinality>
			</owl:Restriction>
		</rdfs:subClassOf>
		<rdfs:subClassOf>
			<owl:Restriction>
				<owl:onProperty rdf:resource="&fibo-fnd-agr-ctr;hasContractParty"/>
				<owl:someValuesFrom rdf:resource="&fibo-fbc-dae-dbt;Borrower"/>
			</owl:Restriction>
		</rdfs:subClassOf>
		<rdfs:subClassOf>
			<owl:Restriction>
				<owl:onProperty rdf:resource="&fibo-fnd-agr-ctr;hasContractParty"/>
				<owl:someValuesFrom rdf:resource="&fibo-fbc-dae-dbt;Lender"/>
			</owl:Restriction>
		</rdfs:subClassOf>
		<rdfs:subClassOf>
			<owl:Restriction>
				<owl:onProperty rdf:resource="&fibo-fnd-rel-rel;has"/>
				<owl:someValuesFrom rdf:resource="&fibo-ln-ln-ln;CreditRiskAssessment"/>
			</owl:Restriction>
		</rdfs:subClassOf>
		<rdfs:subClassOf>
			<owl:Restriction>
				<owl:onProperty rdf:resource="&fibo-fnd-rel-rel;isClassifiedBy"/>
				<owl:someValuesFrom rdf:resource="&fibo-ln-ln-ln;LenderLienPosition"/>
			</owl:Restriction>
		</rdfs:subClassOf>
		<rdfs:subClassOf>
			<owl:Restriction>
				<owl:onProperty rdf:resource="&fibo-fnd-rel-rel;isClassifiedBy"/>
				<owl:someValuesFrom rdf:resource="&fibo-ln-ln-ln;LoanMarketCategory"/>
			</owl:Restriction>
		</rdfs:subClassOf>
		<rdfs:subClassOf>
			<owl:Restriction>
				<owl:onProperty rdf:resource="&fibo-ln-ln-ln;hasBorrower"/>
				<owl:someValuesFrom rdf:resource="&fibo-fnd-pty-pty;IndependentParty"/>
			</owl:Restriction>
		</rdfs:subClassOf>
		<rdfs:subClassOf>
			<owl:Restriction>
				<owl:onProperty rdf:resource="&fibo-ln-ln-ln;hasLender"/>
				<owl:someValuesFrom rdf:resource="&fibo-fnd-pty-pty;IndependentParty"/>
			</owl:Restriction>
		</rdfs:subClassOf>
		<rdfs:subClassOf>
			<owl:Restriction>
				<owl:onProperty rdf:resource="&fibo-ln-ln-ln;hasOriginatorCompany"/>
				<owl:someValuesFrom rdf:resource="&fibo-fnd-org-fm;FormalOrganization"/>
			</owl:Restriction>
		</rdfs:subClassOf>
		<rdfs:subClassOf>
			<owl:Restriction>
				<owl:onProperty rdf:resource="&fibo-ln-ln-ln;hasOriginatorPerson"/>
				<owl:someValuesFrom rdf:resource="&fibo-fnd-aap-ppl;Person"/>
			</owl:Restriction>
		</rdfs:subClassOf>
		<rdfs:subClassOf>
			<owl:Restriction>
				<owl:onProperty rdf:resource="&fibo-ln-ln-up;cur-hasAmount"/>
				<owl:someValuesFrom rdf:resource="&fibo-fnd-acc-cur;MonetaryAmount"/>
			</owl:Restriction>
		</rdfs:subClassOf>
		<rdfs:subClassOf>
			<owl:Restriction>
				<owl:onProperty rdf:resource="&fibo-ln-ln-up;instantiates"/>
				<owl:someValuesFrom rdf:resource="&fibo-ln-ln-ln;LoanOffer"/>
			</owl:Restriction>
		</rdfs:subClassOf>
		<rdfs:subClassOf>
			<owl:Restriction>
				<owl:onProperty rdf:resource="&fibo-ln-ln-up;rel-produces_I"/>
				<owl:someValuesFrom rdf:resource="&fibo-ln-ln-ln;ObligationToFund"/>
			</owl:Restriction>
		</rdfs:subClassOf>
		<skos:definition>An agreement whereby one party extends money or credit to another party with the agreement that the borrowed money will be repaid according to specific terms</skos:definition>
		<fibo-fnd-utl-av:adaptedFrom>http://financial-dictionary.thefreedictionary.com/Loan</fibo-fnd-utl-av:adaptedFrom>
	</owl:Class>
	
	<owl:Class rdf:about="&fibo-ln-ln-ln;LoanMarketCategory">
		<rdfs:subClassOf rdf:resource="&fibo-fnd-arr-cls;Classifier"/>
		<skos:definition>Specifies the market domain in which the loan product is offered.</skos:definition>
	</owl:Class>
	
	<owl:Class rdf:about="&fibo-ln-ln-ln;LoanOffer">
		<rdfs:subClassOf rdf:resource="&fibo-ln-ln-up;pas-Offer"/>
		<rdfs:subClassOf>
			<owl:Restriction>
				<owl:onProperty rdf:resource="&fibo-fnd-rel-rel;has"/>
				<owl:onClass rdf:resource="&fibo-ln-ln-up;pas-LineItem"/>
				<owl:minQualifiedCardinality rdf:datatype="&xs;nonNegativeInteger">0</owl:minQualifiedCardinality>
			</owl:Restriction>
		</rdfs:subClassOf>
		<rdfs:subClassOf>
			<owl:Restriction>
				<owl:onProperty rdf:resource="&fibo-ln-ln-up;hasItemOffered"/>
				<owl:someValuesFrom rdf:resource="&fibo-ln-ln-ln;LoanProduct"/>
			</owl:Restriction>
		</rdfs:subClassOf>
		<skos:definition>A generic loan product offered to the public, or a specific offer tailoered to particular circumstances aimed at one potential borrower.</skos:definition>
	</owl:Class>
	
	<owl:Class rdf:about="&fibo-ln-ln-ln;LoanProduct">
		<rdfs:subClassOf rdf:resource="&fibo-fbc-pas-fpas;FinancialProduct"/>
		<skos:definition>A type of loan that a borrower may acquire from a lending institution with specific characteristics and  terms.</skos:definition>
		<skos:editorialNote>TODO: It may be good to flesh this out a bit, closely related to schema.org.</skos:editorialNote>
	</owl:Class>
	
	<owl:Class rdf:about="&fibo-ln-ln-ln;MortgageLoanContract">
		<rdfs:subClassOf>
			<owl:Restriction>
				<owl:onProperty rdf:resource="&fibo-ln-ln-ln;assumes"/>
				<owl:onClass rdf:resource="&fibo-ln-ln-ln;MortgageLoanContract"/>
				<owl:minQualifiedCardinality rdf:datatype="&xs;nonNegativeInteger">0</owl:minQualifiedCardinality>
			</owl:Restriction>
		</rdfs:subClassOf>
		<rdfs:subClassOf>
			<owl:Restriction>
				<owl:onProperty rdf:resource="&fibo-ln-ln-ln;hasClosingDate"/>
				<owl:someValuesFrom rdf:resource="&fibo-fnd-dt-fd;Date"/>
			</owl:Restriction>
		</rdfs:subClassOf>
		<owl:equivalentClass>
			<owl:Class>
				<owl:intersectionOf rdf:parseType="Collection">
					<rdf:Description rdf:about="&fibo-ln-ln-ln;LoanContract">
					</rdf:Description>
					<owl:Restriction>
						<owl:onProperty rdf:resource="&fibo-fnd-rel-rel;comprises"/>
						<owl:someValuesFrom>
							<owl:Class>
								<owl:intersectionOf rdf:parseType="Collection">
									<rdf:Description rdf:about="&fibo-ln-ln-ln;SecurityAgreement">
									</rdf:Description>
									<owl:Restriction>
										<owl:onProperty rdf:resource="&fibo-ln-ln-ln;hasCollateral"/>
										<owl:someValuesFrom rdf:resource="&fibo-fnd-plc-loc;RealEstate"/>
									</owl:Restriction>
								</owl:intersectionOf>
							</owl:Class>
						</owl:someValuesFrom>
					</owl:Restriction>
				</owl:intersectionOf>
			</owl:Class>
		</owl:equivalentClass>
		<skos:definition>A loan contract that is secured by real property.</skos:definition>
		<fibo-fnd-utl-av:adaptedFrom>the Cambridge Business English Dictionary</fibo-fnd-utl-av:adaptedFrom>
	</owl:Class>
	
	<owl:Class rdf:about="&fibo-ln-ln-ln;MortgageLoanPurpose">
		<rdfs:subClassOf rdf:resource="&fibo-fnd-arr-cls;Classifier"/>
		<skos:definition>The purpose for which mortgage loan proceeds will be used such as real property purchase, dwelling construction, or loan refinancing.</skos:definition>
	</owl:Class>
	
	<owl:Class rdf:about="&fibo-ln-ln-ln;ObligationToFund">
		<rdfs:subClassOf rdf:resource="&fibo-ln-ln-ln;ObligationToPay"/>
		<skos:definition>An obligation of the Lender to provide funds pursuant to a loan contract.</skos:definition>
	</owl:Class>
	
	<owl:Class rdf:about="&fibo-ln-ln-ln;ObligationToPay">
		<rdfs:subClassOf rdf:resource="&fibo-fnd-agr-agr;Commitment"/>
		<rdfs:subClassOf>
			<owl:Restriction>
				<owl:onProperty rdf:resource="&fibo-fnd-rel-rel;has"/>
				<owl:someValuesFrom rdf:resource="&fibo-ln-ln-up;pas-LineItem"/>
			</owl:Restriction>
		</rdfs:subClassOf>
		<rdfs:subClassOf>
			<owl:Restriction>
				<owl:onProperty rdf:resource="&fibo-ln-ln-up;hasPayee"/>
				<owl:someValuesFrom rdf:resource="&fibo-fnd-pty-pty;IndependentParty"/>
			</owl:Restriction>
		</rdfs:subClassOf>
		<rdfs:subClassOf>
			<owl:Restriction>
				<owl:onProperty rdf:resource="&fibo-ln-ln-up;hasPayor"/>
				<owl:someValuesFrom rdf:resource="&fibo-fnd-pty-pty;IndependentParty"/>
			</owl:Restriction>
		</rdfs:subClassOf>
		<skos:definition>An obligation for one party to make a payment to another party.  E.g. to fund a loan, make payments, pay origination fees.</skos:definition>
		<skos:editorialNote>TODO: consider adding payment methods, and timing constraints.</skos:editorialNote>
	</owl:Class>
	
	<owl:Class rdf:about="&fibo-ln-ln-ln;ObligationToRepay">
		<rdfs:subClassOf rdf:resource="&fibo-ln-ln-ln;ObligationToPay"/>
		<rdfs:subClassOf>
			<owl:Restriction>
				<owl:onProperty rdf:resource="&fibo-fnd-rel-rel;has"/>
				<owl:someValuesFrom rdf:resource="&fibo-ln-ln-up;PaymentHistory"/>
			</owl:Restriction>
		</rdfs:subClassOf>
		<rdfs:subClassOf>
			<owl:Restriction>
				<owl:onProperty rdf:resource="&fibo-fnd-rel-rel;has"/>
				<owl:someValuesFrom rdf:resource="&fibo-ln-ln-up;PaymentSchedule"/>
			</owl:Restriction>
		</rdfs:subClassOf>
		<skos:definition>An obligation of the Borrower to repay funds that have been loaned, in a manner pursuant to a loan contract.</skos:definition>
	</owl:Class>
	
	<owl:Class rdf:about="&fibo-ln-ln-ln;ObligationToReport">
		<rdfs:subClassOf rdf:resource="&fibo-fnd-agr-agr;Commitment"/>
		<skos:definition>Obligation to report to some IndependentParty.</skos:definition>
	</owl:Class>
	
	<owl:Class rdf:about="&fibo-ln-ln-ln;OpenEndLoanContract">
		<rdfs:subClassOf rdf:resource="&fibo-ln-ln-ln;LoanContract"/>
		<rdfs:subClassOf>
			<owl:Restriction>
				<owl:onProperty rdf:resource="&fibo-ln-ln-ln;hasCreditLimit"/>
				<owl:someValuesFrom rdf:resource="&fibo-fnd-acc-cur;MonetaryAmount"/>
			</owl:Restriction>
		</rdfs:subClassOf>
		<skos:definition>A LoanContract for a line of credit where a borrower may take money and pay it back up to an agreed limit, and interest is charged only on the amount that remains, which may be paid off at any time within the period of the line.</skos:definition>
		<fibo-fnd-utl-av:adaptedFrom>Cambridge Business English Dictionary.</fibo-fnd-utl-av:adaptedFrom>
	</owl:Class>
	
	<owl:Class rdf:about="&fibo-ln-ln-ln;PreApprovalContract">
		<rdfs:subClassOf rdf:resource="&fibo-fnd-agr-ctr;WrittenContract"/>
		<rdfs:subClassOf>
			<owl:Restriction>
				<owl:onProperty rdf:resource="&fibo-fbc-dae-dbt;hasInterestRate"/>
				<owl:someValuesFrom rdf:resource="&fibo-fnd-acc-cur;InterestRate"/>
			</owl:Restriction>
		</rdfs:subClassOf>
		<rdfs:subClassOf>
			<owl:Restriction>
				<owl:onProperty rdf:resource="&fibo-ln-ln-ln;hasApprovedAmount"/>
				<owl:someValuesFrom rdf:resource="&fibo-fnd-acc-cur;MonetaryAmount"/>
			</owl:Restriction>
		</rdfs:subClassOf>
		<skos:definition>A written commitment to lend when specified conditions are met, e.g. finding suitable property, and unchanged creditworthiness.</skos:definition>
		<fibo-fnd-utl-av:adaptedFrom>the 2015 Revised HMDA regulation.</fibo-fnd-utl-av:adaptedFrom>
		<fibo-fnd-utl-av:explanatoryNote>A commitment from a lender to a borrower to extend a home purchase loan up to a certain amount, and subject to certain non-credit related conditions.  This commitment is entered into after a comprehensive analysis of the credit worthiness of the borrower is carried out.</fibo-fnd-utl-av:explanatoryNote>
		<fibo-fnd-utl-av:explanatoryNote>NOTE: this may also include limits on the region where to purchase.</fibo-fnd-utl-av:explanatoryNote>
	</owl:Class>
	
	<owl:Class rdf:about="&fibo-ln-ln-ln;PreApprovalRequest">
		<rdfs:subClassOf rdf:resource="&fibo-ln-ln-up;fnd-Request"/>
		<rdfs:subClassOf>
			<owl:Restriction>
				<owl:onProperty rdf:resource="&fibo-ln-ln-ln;hasBorrower"/>
				<owl:someValuesFrom rdf:resource="&fibo-fnd-pty-pty;IndependentParty"/>
			</owl:Restriction>
		</rdfs:subClassOf>
		<rdfs:subClassOf>
			<owl:Restriction>
				<owl:onProperty rdf:resource="&fibo-ln-ln-ln;hasRequestedAmount"/>
				<owl:someValuesFrom rdf:resource="&fibo-fnd-acc-cur;MonetaryAmount"/>
			</owl:Restriction>
		</rdfs:subClassOf>
		<skos:definition>request from a potential borrower that a lender commit to pre-approving the borrower for a loan of up to a specified amount of money.</skos:definition>
		<fibo-fnd-utl-av:explanatoryNote>NOTE: this may also inlcude limits on the region where to purchase.</fibo-fnd-utl-av:explanatoryNote>
	</owl:Class>
	
	<owl:Class rdf:about="&fibo-ln-ln-ln;PropertyInspection">
		<rdfs:subClassOf rdf:resource="&fibo-fnd-dt-oc;Occurrence"/>
		<rdfs:subClassOf>
			<owl:Restriction>
				<owl:onProperty rdf:resource="&fibo-ln-ln-ln;hasItemInspected"/>
				<owl:onClass rdf:resource="&fibo-fnd-plc-loc;RealEstate"/>
				<owl:minQualifiedCardinality rdf:datatype="&xs;nonNegativeInteger">1</owl:minQualifiedCardinality>
			</owl:Restriction>
		</rdfs:subClassOf>
		<rdfs:subClassOf>
			<owl:Restriction>
				<owl:onProperty rdf:resource="&fibo-ln-ln-up;performedBy"/>
				<owl:someValuesFrom rdf:resource="&fibo-fnd-pty-pty;IndependentParty"/>
			</owl:Restriction>
		</rdfs:subClassOf>
		<skos:definition>The act of analyzing one or more aspects of a real property for independent assessment of status or deficiency.</skos:definition>
		<fibo-fnd-utl-av:explanatoryNote>This is independent and separate from conducting an appraisal. Examples are termite inspections, construction inspections, etc.</fibo-fnd-utl-av:explanatoryNote>
	</owl:Class>
	
	<owl:Class rdf:about="&fibo-ln-ln-ln;PropertyUsage">
		<rdfs:subClassOf rdf:resource="&fibo-fnd-arr-cls;Classifier"/>
		<skos:definition>A category for the manner in which the borrower intends to utilize the property.</skos:definition>
	</owl:Class>
	
	<owl:Class rdf:about="&fibo-ln-ln-ln;PublicRecord">
		<rdfs:subClassOf rdf:resource="&fibo-ln-ln-up;Report"/>
		<rdfs:subClassOf>
			<owl:Restriction>
				<owl:onProperty rdf:resource="&fibo-fnd-rel-rel;refersTo"/>
				<owl:onClass rdf:resource="&fibo-fbc-pas-caa;Account"/>
				<owl:minQualifiedCardinality rdf:datatype="&xs;nonNegativeInteger">0</owl:minQualifiedCardinality>
			</owl:Restriction>
		</rdfs:subClassOf>
		<rdfs:subClassOf>
			<owl:Restriction>
				<owl:onProperty rdf:resource="&fibo-ln-ln-up;isEvidencedBy_g"/>
				<owl:onClass rdf:resource="&fibo-fnd-arr-doc;LegalDocument"/>
				<owl:minQualifiedCardinality rdf:datatype="&xs;nonNegativeInteger">0</owl:minQualifiedCardinality>
			</owl:Restriction>
		</rdfs:subClassOf>
		<rdfs:subClassOf>
			<owl:Restriction>
				<owl:onProperty rdf:resource="&fibo-fnd-rel-rel;isClassifiedBy"/>
				<owl:someValuesFrom rdf:resource="&fibo-ln-ln-ln;PublicRecordCategory"/>
			</owl:Restriction>
		</rdfs:subClassOf>
		<skos:definition>A record about an action involving a party that is publicly available from court or other government agencies.  This can include court actions such as bankruptcy and foreclosure, as well as liens and other events that have been recorded.</skos:definition>
		<skos:editorialNote>This assumes that the domain of the property refersTo has been removed.  At one point it was such that the PublicRecord is  incorrectly infered  into the class Reference.</skos:editorialNote>
	</owl:Class>
	
	<owl:Class rdf:about="&fibo-ln-ln-ln;PublicRecordCategory">
		<rdfs:subClassOf rdf:resource="&fibo-fnd-arr-cls;Classifier"/>
		<skos:definition>A particular classification of public record, e.g. tax lien, wage garnishment, foreclosure.</skos:definition>
	</owl:Class>
	
	<owl:Class rdf:about="&fibo-ln-ln-ln;Race">
		<rdfs:subClassOf>
			<owl:Restriction>
				<owl:onProperty rdf:resource="&skos;broaderTransitive"/>
				<owl:someValuesFrom rdf:resource="&fibo-ln-ln-ln;Race"/>
			</owl:Restriction>
		</rdfs:subClassOf>
		<rdfs:subClassOf>
			<owl:Restriction>
				<owl:onProperty rdf:resource="&fibo-fnd-rel-rel;classifies"/>
				<owl:someValuesFrom rdf:resource="&fibo-fnd-aap-ppl;Person"/>
			</owl:Restriction>
		</rdfs:subClassOf>
		<skos:definition>A category based on a person&apos;s physical characteristics, such as bone structure and skin, hair, or eye color.</skos:definition>
	</owl:Class>
	
	<owl:Class rdf:about="&fibo-ln-ln-ln;RealPropertyAppraisal">
		<rdfs:subClassOf rdf:resource="&fibo-ln-ln-up;Valuation"/>
		<rdfs:subClassOf>
			<owl:Restriction>
				<owl:onProperty rdf:resource="&fibo-ln-ln-up;rel-isInformedBy"/>
				<owl:onClass rdf:resource="&fibo-ln-ln-ln;PropertyInspection"/>
				<owl:minQualifiedCardinality rdf:datatype="&xs;nonNegativeInteger">0</owl:minQualifiedCardinality>
			</owl:Restriction>
		</rdfs:subClassOf>
		<rdfs:subClassOf>
			<owl:Restriction>
				<owl:onProperty rdf:resource="&fibo-fnd-dt-fd;hasDate"/>
				<owl:someValuesFrom rdf:resource="&fibo-fnd-dt-fd;Date"/>
			</owl:Restriction>
		</rdfs:subClassOf>
		<rdfs:subClassOf>
			<owl:Restriction>
				<owl:onProperty rdf:resource="&fibo-ln-ln-ln;hasAppraisalManagementCompany"/>
				<owl:someValuesFrom rdf:resource="&fibo-fnd-pty-pty;IndependentParty"/>
			</owl:Restriction>
		</rdfs:subClassOf>
		<rdfs:subClassOf>
			<owl:Restriction>
				<owl:onProperty rdf:resource="&fibo-ln-ln-ln;hasAppraisedValue"/>
				<owl:someValuesFrom rdf:resource="&fibo-fnd-acc-cur;MonetaryAmount"/>
			</owl:Restriction>
		</rdfs:subClassOf>
		<rdfs:subClassOf>
			<owl:Restriction>
				<owl:onProperty rdf:resource="&fibo-ln-ln-up;hasAppraiser"/>
				<owl:someValuesFrom rdf:resource="&fibo-fnd-pty-pty;IndependentParty"/>
			</owl:Restriction>
		</rdfs:subClassOf>
		<rdfs:subClassOf>
			<owl:Restriction>
				<owl:onProperty rdf:resource="&fibo-ln-ln-up;hasSeniorAppraiser"/>
				<owl:someValuesFrom rdf:resource="&fibo-fnd-pty-pty;IndependentParty"/>
			</owl:Restriction>
		</rdfs:subClassOf>
		<skos:definition>An act of real estate valuation conducted by an appraiser or technology with a logical model that performs the same function. Valuation determines the amount of money a real estate property is worth, through one or more methodologies.</skos:definition>
		<skos:editorialNote>TODO: Maybe add superclass called Evaluation and include information about variability analysis and maybe the algorithm used.</skos:editorialNote>
		<fibo-fnd-utl-av:usageNote>Ensure that the appraiser parties have NMLS Identifier and contact preferences, e.g. phone number and address.

As needed, use the worksFor property to connect appraisers to the appraisal management company.</fibo-fnd-utl-av:usageNote>
	</owl:Class>
	
	<owl:Class rdf:about="&fibo-ln-ln-ln;ReverseMortgageLoanContract">
		<rdfs:subClassOf rdf:resource="&fibo-ln-ln-ln;MortgageLoanContract"/>
		<rdfs:subClassOf>
			<owl:Restriction>
				<owl:onProperty rdf:resource="&fibo-ln-ln-ln;hasCreditLimit"/>
				<owl:someValuesFrom rdf:resource="&fibo-fnd-acc-cur;MonetaryAmount"/>
			</owl:Restriction>
		</rdfs:subClassOf>
		<skos:definition>A mortgage contract that pays out money to the borrower against a set principal limit that is based on the value of existing equity in the underlying collateral.  The interest is added to the principal balance.</skos:definition>
		<fibo-fnd-utl-av:explanatoryNote>Note that a reverse mortgage and an open end loan both have a credit limit.</fibo-fnd-utl-av:explanatoryNote>
	</owl:Class>
	
	<owl:Class rdf:about="&fibo-ln-ln-ln;SecuredLoanContract">
		<owl:equivalentClass>
			<owl:Class>
				<owl:intersectionOf rdf:parseType="Collection">
					<rdf:Description rdf:about="&fibo-ln-ln-ln;LoanContract">
					</rdf:Description>
					<owl:Restriction>
						<owl:onProperty rdf:resource="&fibo-fnd-rel-rel;hasPart"/>
						<owl:someValuesFrom rdf:resource="&fibo-ln-ln-ln;SecurityAgreement"/>
					</owl:Restriction>
				</owl:intersectionOf>
			</owl:Class>
		</owl:equivalentClass>
		<skos:definition>A loan contract that is secured by some collateral.</skos:definition>
	</owl:Class>
	
	<owl:Class rdf:about="&fibo-ln-ln-ln;SecurityAgreement">
		<rdfs:subClassOf>
			<owl:Restriction>
				<owl:onProperty rdf:resource="&fibo-fnd-rel-rel;isClassifiedBy"/>
				<owl:someValuesFrom rdf:resource="&fibo-ln-ln-ln;LenderLienPosition"/>
			</owl:Restriction>
		</rdfs:subClassOf>
		<rdfs:subClassOf>
			<owl:Restriction>
				<owl:onProperty rdf:resource="&fibo-fnd-rel-rel;isPartOf"/>
				<owl:someValuesFrom rdf:resource="&fibo-ln-ln-ln;LoanContract"/>
			</owl:Restriction>
		</rdfs:subClassOf>
		<owl:equivalentClass>
			<owl:Class>
				<owl:intersectionOf rdf:parseType="Collection">
					<rdf:Description rdf:about="&fibo-fnd-agr-ctr;WrittenContract">
					</rdf:Description>
					<owl:Restriction>
						<owl:onProperty rdf:resource="&fibo-ln-ln-ln;hasCollateral"/>
						<owl:someValuesFrom>
							<owl:Class>
								<owl:intersectionOf rdf:parseType="Collection">
									<owl:Restriction>
										<owl:onProperty rdf:resource="&fibo-ln-ln-up;cur-hasEstimatedValue"/>
										<owl:someValuesFrom rdf:resource="&fibo-fnd-acc-cur;MonetaryAmount"/>
									</owl:Restriction>
									<owl:Restriction>
										<owl:onProperty rdf:resource="&fibo-fnd-oac-own;isOwnedBy"/>
										<owl:someValuesFrom rdf:resource="&fibo-fnd-pty-pty;IndependentParty"/>
									</owl:Restriction>
								</owl:intersectionOf>
							</owl:Class>
						</owl:someValuesFrom>
					</owl:Restriction>
				</owl:intersectionOf>
			</owl:Class>
		</owl:equivalentClass>
		<skos:definition>Agreement between two trading parties that contains information about their relative duties and rights regarding the disposition of a specified asset that has been used as collateral.</skos:definition>
		<fibo-fnd-utl-av:adaptedFrom>ISO 20022</fibo-fnd-utl-av:adaptedFrom>
		<fibo-fnd-utl-av:explanatoryNote>NOTE: Collateral is more than just an economic resource, it has to in fact be owned. Hence it is an Asset.</fibo-fnd-utl-av:explanatoryNote>
	</owl:Class>
	
	<owl:Class rdf:about="&fibo-ln-ln-ln;UniversalLoanIdentifier">
		<rdfs:subClassOf rdf:resource="&fibo-fbc-fi-fi;FinancialInstrumentIdentifier"/>
		<rdfs:subClassOf>
			<owl:Restriction>
				<owl:onProperty rdf:resource="&fibo-fnd-rel-rel;comprises"/>
				<owl:onClass rdf:resource="&fibo-be-le-lei;LegalEntityIdentifier"/>
				<owl:qualifiedCardinality rdf:datatype="&xs;nonNegativeInteger">1</owl:qualifiedCardinality>
			</owl:Restriction>
		</rdfs:subClassOf>
		<rdfs:subClassOf>
			<owl:Restriction>
				<owl:onProperty rdf:resource="&fibo-fnd-aap-agt;identifies"/>
				<owl:onClass rdf:resource="&fibo-ln-ln-ln;LoanContract"/>
				<owl:qualifiedCardinality rdf:datatype="&xs;nonNegativeInteger">1</owl:qualifiedCardinality>
			</owl:Restriction>
		</rdfs:subClassOf>
		<skos:definition>A unique identifier given to unequivocally identify a specific mortgage loan.  In the US, the structure of this identifier is defined in the 2015 revision to the Home Mortgage Disclosure Act.</skos:definition>
	</owl:Class>
	
	<fibo-ln-ln-ln:CreditInquiryType rdf:about="&fibo-ln-ln-ln;_CreditInquiryType_hard">
	</fibo-ln-ln-ln:CreditInquiryType>
	
	<fibo-ln-ln-ln:CreditInquiryType rdf:about="&fibo-ln-ln-ln;_CreditInquiryType_soft">
	</fibo-ln-ln-ln:CreditInquiryType>
	
	<fibo-ln-ln-ln:CreditMessageType rdf:about="&fibo-ln-ln-ln;_CreditMessage_alert">
	</fibo-ln-ln-ln:CreditMessageType>
	
	<fibo-ln-ln-ln:CreditMessageType rdf:about="&fibo-ln-ln-ln;_CreditMessage_freeze">
	</fibo-ln-ln-ln:CreditMessageType>
	
	<fibo-ln-ln-ln:CreditScoreModelType rdf:about="&fibo-ln-ln-ln;_CreditModel_cm1">
	</fibo-ln-ln-ln:CreditScoreModelType>
	
	<fibo-ln-ln-ln:CreditScoreModelType rdf:about="&fibo-ln-ln-ln;_CreditModel_cm2">
	</fibo-ln-ln-ln:CreditScoreModelType>
	
	<fibo-ln-ln-ln:IsPreApprovalRequested rdf:about="&fibo-ln-ln-ln;_IsPreApprovalRequested_NO">
	</fibo-ln-ln-ln:IsPreApprovalRequested>
	
	<fibo-ln-ln-ln:IsPreApprovalRequested rdf:about="&fibo-ln-ln-ln;_IsPreApprovalRequested_YES">
	</fibo-ln-ln-ln:IsPreApprovalRequested>
	
	<fibo-ln-ln-ln:LenderLienPosition rdf:about="&fibo-ln-ln-ln;_LienPosition_primary">
	</fibo-ln-ln-ln:LenderLienPosition>
	
	<fibo-ln-ln-ln:LenderLienPosition rdf:about="&fibo-ln-ln-ln;_LienPosition_subordinate">
	</fibo-ln-ln-ln:LenderLienPosition>
	
	<fibo-ln-ln-ln:LoanMarketCategory rdf:about="&fibo-ln-ln-ln;_LoanMarketCategory_Automobile">
	</fibo-ln-ln-ln:LoanMarketCategory>
	
	<fibo-ln-ln-ln:LoanMarketCategory rdf:about="&fibo-ln-ln-ln;_LoanMarketCategory_Commercial">
	</fibo-ln-ln-ln:LoanMarketCategory>
	
	<fibo-ln-ln-ln:LoanMarketCategory rdf:about="&fibo-ln-ln-ln;_LoanMarketCategory_Construction">
	</fibo-ln-ln-ln:LoanMarketCategory>
	
	<fibo-ln-ln-ln:LoanMarketCategory rdf:about="&fibo-ln-ln-ln;_LoanMarketCategory_Education">
	</fibo-ln-ln-ln:LoanMarketCategory>
	
	<fibo-ln-ln-ln:LoanMarketCategory rdf:about="&fibo-ln-ln-ln;_LoanMarketCategory_Mortgage">
	</fibo-ln-ln-ln:LoanMarketCategory>
	
	<fibo-ln-ln-ln:LoanMarketCategory rdf:about="&fibo-ln-ln-ln;_LoanMarketCategory_Personal">
	</fibo-ln-ln-ln:LoanMarketCategory>
	
	<fibo-ln-ln-ln:LoanMarketCategory rdf:about="&fibo-ln-ln-ln;_LoanMarketCategory_SmallBusiness">
	</fibo-ln-ln-ln:LoanMarketCategory>
	
	<fibo-ln-ln-ln:PublicRecordCategory rdf:about="&fibo-ln-ln-ln;_PublicRecordCategory_bankruptcy">
	</fibo-ln-ln-ln:PublicRecordCategory>
	
	<fibo-ln-ln-ln:PublicRecordCategory rdf:about="&fibo-ln-ln-ln;_PublicRecordCategory_civilOrJudgement">
	</fibo-ln-ln-ln:PublicRecordCategory>
	
	<fibo-ln-ln-ln:PublicRecordCategory rdf:about="&fibo-ln-ln-ln;_PublicRecordCategory_foreclosure">
	</fibo-ln-ln-ln:PublicRecordCategory>
	
	<fibo-ln-ln-ln:PublicRecordCategory rdf:about="&fibo-ln-ln-ln;_PublicRecordCategory_garnishment">
	</fibo-ln-ln-ln:PublicRecordCategory>
	
	<fibo-ln-ln-ln:PublicRecordCategory rdf:about="&fibo-ln-ln-ln;_PublicRecordCategory_lien">
	</fibo-ln-ln-ln:PublicRecordCategory>
	
	<fibo-ln-ln-ln:PublicRecordCategory rdf:about="&fibo-ln-ln-ln;_PublicRecordCategory_marital">
	</fibo-ln-ln-ln:PublicRecordCategory>
	
	<fibo-ln-ln-ln:PublicRecordCategory rdf:about="&fibo-ln-ln-ln;_PublicRecordCategory_personalProperty">
	</fibo-ln-ln-ln:PublicRecordCategory>
	
	<fibo-ln-ln-ln:PublicRecordCategory rdf:about="&fibo-ln-ln-ln;_PublicRecordCategory_realEstate">
	</fibo-ln-ln-ln:PublicRecordCategory>
	
	<fibo-ln-ln-ln:CashOutStatus rdf:about="&fibo-ln-ln-ln;_cashOutStatus_CashOut">
		<rdf:type rdf:resource="&owl;Thing"/>
		<skos:definition>Lynn todo:</skos:definition>
	</fibo-ln-ln-ln:CashOutStatus>
	
	<fibo-ln-ln-ln:CashOutStatus rdf:about="&fibo-ln-ln-ln;_cashOutStatus_LimitedCashOut">
		<rdf:type rdf:resource="&owl;Thing"/>
		<skos:definition>Lynn todo:</skos:definition>
	</fibo-ln-ln-ln:CashOutStatus>
	
	<fibo-ln-ln-ln:CashOutStatus rdf:about="&fibo-ln-ln-ln;_cashOutStatus_NoCashOut">
		<rdf:type rdf:resource="&owl;Thing"/>
		<skos:definition>Lynn todo:</skos:definition>
	</fibo-ln-ln-ln:CashOutStatus>
	
	<fibo-ln-ln-ln:PropertyUsage rdf:about="&fibo-ln-ln-ln;_investment">
		<rdf:type rdf:resource="&owl;Thing"/>
		<skos:definition>A home owned for the purpose of generating income.</skos:definition>
	</fibo-ln-ln-ln:PropertyUsage>
	
	<fibo-ln-ln-ln:ConstructionType rdf:about="&fibo-ln-ln-ln;_manufactured">
		<rdf:type rdf:resource="&owl;Thing"/>
		<skos:definition>A factory built dwelling built in compliance with the Federal Manufactured Home Construction and Safety Standards in effect at the time the home was manufactured as evidenced by the HUD label.</skos:definition>
	</fibo-ln-ln-ln:ConstructionType>
	
	<fibo-ln-ln-ln:ConstructionType rdf:about="&fibo-ln-ln-ln;_mobileHome">
		<rdf:type rdf:resource="&owl;Thing"/>
		<skos:definition>Dwelling unit constructed on a base frame which features wheels and axles to be used in transporting home from place to place, does not meet HUD code.</skos:definition>
	</fibo-ln-ln-ln:ConstructionType>
	
	<fibo-ln-ln-ln:ConstructionType rdf:about="&fibo-ln-ln-ln;_modular">
		<rdf:type rdf:resource="&owl;Thing"/>
		<skos:definition>A factory built dwelling not on a permanent chassis.</skos:definition>
	</fibo-ln-ln-ln:ConstructionType>
	
	<fibo-ln-ln-ln:MortgageLoanPurpose rdf:about="&fibo-ln-ln-ln;_mortgageLoanPurpose_DwellingConstruction">
	</fibo-ln-ln-ln:MortgageLoanPurpose>
	
	<fibo-ln-ln-ln:MortgageLoanPurpose rdf:about="&fibo-ln-ln-ln;_mortgageLoanPurpose_HomeImprovement">
	</fibo-ln-ln-ln:MortgageLoanPurpose>
	
	<fibo-ln-ln-ln:MortgageLoanPurpose rdf:about="&fibo-ln-ln-ln;_mortgageLoanPurpose_LoanRefinancing">
	</fibo-ln-ln-ln:MortgageLoanPurpose>
	
	<fibo-ln-ln-ln:MortgageLoanPurpose rdf:about="&fibo-ln-ln-ln;_mortgageLoanPurpose_MortgageModification">
	</fibo-ln-ln-ln:MortgageLoanPurpose>
	
	<fibo-ln-ln-ln:MortgageLoanPurpose rdf:about="&fibo-ln-ln-ln;_mortgageLoanPurpose_RealPropertyPurchase">
	</fibo-ln-ln-ln:MortgageLoanPurpose>
	
	<fibo-ln-ln-ln:DwellingCapacity rdf:about="&fibo-ln-ln-ln;_multiFamily">
		<rdf:type rdf:resource="&owl;Thing"/>
		<skos:definition>5 or more units</skos:definition>
	</fibo-ln-ln-ln:DwellingCapacity>
	
	<fibo-ln-ln-ln:ConstructionType rdf:about="&fibo-ln-ln-ln;_onFrameModular">
		<rdf:type rdf:resource="&owl;Thing"/>
		<skos:definition>A factory built dwelling on a permanent chassis which does not have a HUD label.</skos:definition>
	</fibo-ln-ln-ln:ConstructionType>
	
	<fibo-ln-ln-ln:PropertyUsage rdf:about="&fibo-ln-ln-ln;_primaryResidence">
		<rdf:type rdf:resource="&owl;Thing"/>
		<skos:definition>Residence that the owner physically occupies and uses as his or her principal residence.</skos:definition>
	</fibo-ln-ln-ln:PropertyUsage>
	
	<fibo-ln-ln-ln:PropertyUsage rdf:about="&fibo-ln-ln-ln;_secondHome">
		<rdf:type rdf:resource="&owl;Thing"/>
		<skos:definition>A property occupied by the owner for a portion of the year that is not the primary residence.</skos:definition>
	</fibo-ln-ln-ln:PropertyUsage>
	
	<fibo-ln-ln-ln:DwellingCapacity rdf:about="&fibo-ln-ln-ln;_singleFamily">
		<rdf:type rdf:resource="&owl;Thing"/>
		<skos:definition>1-4 units</skos:definition>
	</fibo-ln-ln-ln:DwellingCapacity>
	
	<fibo-ln-ln-ln:ConstructionType rdf:about="&fibo-ln-ln-ln;_siteBuilt">
		<rdf:type rdf:resource="&owl;Thing"/>
		<skos:definition>Describes construction process, indicating that most elements are created at the homes permanent site. May include some prefabricated components.</skos:definition>
	</fibo-ln-ln-ln:ConstructionType>
	
	<owl:ObjectProperty rdf:about="&fibo-ln-ln-ln;assumes">
		<skos:definition>Relates a new mortgage loan contract to a previous one made to a different borrower for the same property. The new contract is created via a legally binding process where the new borrower assumes the terms of the previous loan contract.</skos:definition>
	</owl:ObjectProperty>
	
	<owl:ObjectProperty rdf:about="&fibo-ln-ln-ln;hasAppraisalManagementCompany">
		<rdfs:subPropertyOf rdf:resource="&fibo-fnd-pty-pty;hasParty"/>
		<skos:definition>Relates something to an independent entity through which mortgage lenders order residential real estate valuation services for properties on which they are considering extending loans to homebuyers, as required by US law.</skos:definition>
		<skos:editorialNote>Broaden to beyond US only.</skos:editorialNote>
		<fibo-fnd-utl-av:definitionOrigin>Investopedia</fibo-fnd-utl-av:definitionOrigin>
	</owl:ObjectProperty>
	
	<owl:ObjectProperty rdf:about="&fibo-ln-ln-ln;hasAppraisedValue">
		<rdfs:subPropertyOf rdf:resource="&fibo-fnd-acc-cur;hasNotionalAmount"/>
		<skos:definition>Relates to a monetary amount that is the product of a valuation process</skos:definition>
		<skos:editorialNote>This should be a subproperty of the property that ties a Valuation to a MonetaryAmount.</skos:editorialNote>
	</owl:ObjectProperty>
	
	<owl:ObjectProperty rdf:about="&fibo-ln-ln-ln;hasApprovedAmount">
		<rdfs:subPropertyOf rdf:resource="&fibo-ln-ln-up;cur-hasAmount"/>
		<skos:definition>Relates, e.g. a loan,  to the amount of funds approved.</skos:definition>
	</owl:ObjectProperty>
	
	<owl:ObjectProperty rdf:about="&fibo-ln-ln-ln;hasBorrower">
		<rdfs:subPropertyOf rdf:resource="&fibo-fnd-pty-pty;hasParty"/>
		<skos:definition>Relates something to an actual or potential borrower. .e.g. a LoanContract to the borrowing party, or a CreditInquiry to a potential borrower.</skos:definition>
	</owl:ObjectProperty>
	
	<owl:ObjectProperty rdf:about="&fibo-ln-ln-ln;hasClosingDate">
		<rdfs:subPropertyOf rdf:resource="&fibo-fnd-agr-ctr;hasEffectiveDate"/>
		<skos:definition>Relates, e.g. a loan contract to the date on which the contract is consummated, officially creating the obligations therein.</skos:definition>
	</owl:ObjectProperty>
	
	<owl:ObjectProperty rdf:about="&fibo-ln-ln-ln;hasCollateral">
		<rdfs:subPropertyOf rdf:resource="&fibo-ln-ln-up;hasParticipant"/>
		<skos:definition>Relates a collateral agreement to an Asset to which title has been taken in security for a loan.</skos:definition>
	</owl:ObjectProperty>
	
	<owl:ObjectProperty rdf:about="&fibo-ln-ln-ln;hasCoveragePeriod">
		<rdfs:subPropertyOf rdf:resource="&fibo-fnd-dt-fd;hasDatePeriod"/>
		<rdfs:comment>relates something (e.g. a report or policy)  to the date period which it covers.</rdfs:comment>
		<rdfs:range rdf:resource="&fibo-fnd-dt-fd;DatePeriod"/>
		<skos:definition>relates something (e.g. a credit report or insurance policy) to the specific time period that it covers</skos:definition>
		<fibo-fnd-utl-av:adaptedFrom>http://www.investopedia.com/terms/t/termlife.asp</fibo-fnd-utl-av:adaptedFrom>
	</owl:ObjectProperty>
	
	<owl:ObjectProperty rdf:about="&fibo-ln-ln-ln;hasCreditLimit">
		<rdfs:subPropertyOf rdf:resource="&fibo-ln-ln-up;cur-hasAmount"/>
		<skos:definition>Relates to the maximum amount of funds that may be borrowed from an account (e.g. for line of credit).</skos:definition>
	</owl:ObjectProperty>
	
	<owl:ObjectProperty rdf:about="&fibo-ln-ln-ln;hasCreditReportingAgency">
		<rdfs:subPropertyOf rdf:resource="&fibo-fnd-pty-pty;hasParty"/>
		<skos:definition>Relates something to a party which is prodiving credit report(s) e.g. needed to assess the risk of a loan</skos:definition>
	</owl:ObjectProperty>
	
	<owl:ObjectProperty rdf:about="&fibo-ln-ln-ln;hasItemInspected">
		<rdfs:subPropertyOf rdf:resource="&fibo-ln-ln-up;hasParticipant"/>
		<skos:definition>Relates an Inspection to the thing being inspected.</skos:definition>
	</owl:ObjectProperty>
	
	<owl:ObjectProperty rdf:about="&fibo-ln-ln-ln;hasLender">
		<rdfs:subPropertyOf rdf:resource="&fibo-fnd-pty-pty;hasParty"/>
		<skos:definition>Relates something to an actual or potential lender. .e.g. a LoanContract to the lending party, or a pre-approval request to a potential lender.</skos:definition>
	</owl:ObjectProperty>
	
	<owl:ObjectProperty rdf:about="&fibo-ln-ln-ln;hasNoteAmount">
		<rdfs:subPropertyOf rdf:resource="&fibo-ln-ln-up;cur-hasAmount"/>
		<skos:definition>Relates something to an amount to be paid as specified on an executed promissory note.</skos:definition>
	</owl:ObjectProperty>
	
	<owl:ObjectProperty rdf:about="&fibo-ln-ln-ln;hasOriginatorCompany">
		<rdfs:subPropertyOf rdf:resource="&fibo-fnd-pty-pty;hasParty"/>
		<rdfs:range rdf:resource="&fibo-fnd-org-org;Organization"/>
		<skos:definition>Relates something, typically  a loan contract, to the  company affilliated with the person originating the loan.</skos:definition>
	</owl:ObjectProperty>
	
	<owl:ObjectProperty rdf:about="&fibo-ln-ln-ln;hasOriginatorPerson">
		<rdfs:subPropertyOf rdf:resource="&fibo-fnd-pty-pty;hasParty"/>
		<rdfs:range rdf:resource="&fibo-fnd-aap-ppl;Person"/>
		<skos:definition>Relates something, typically  a loan contract, to a person that initially originates or creates it.</skos:definition>
	</owl:ObjectProperty>
	
	<owl:ObjectProperty rdf:about="&fibo-ln-ln-ln;hasPartyBeingChecked">
		<rdfs:subPropertyOf rdf:resource="&fibo-fnd-pty-pty;hasParty"/>
		<skos:definition>Is a party for which a credit report is being or has been requested</skos:definition>
	</owl:ObjectProperty>
	
	<owl:ObjectProperty rdf:about="&fibo-ln-ln-ln;hasRequestedAmount">
		<rdfs:subPropertyOf rdf:resource="&fibo-ln-ln-up;cur-hasAmount"/>
		<skos:definition>Relates e.g. a request for a loan  to the amount of funds requested (e.g. regarding a loan)</skos:definition>
	</owl:ObjectProperty>

</rdf:RDF>