<?xml version="1.0" encoding="UTF-8"?>
<!DOCTYPE rdf:RDF [
	<!ENTITY dct "http://purl.org/dc/terms/">
	<!ENTITY fibo-be-le-fbo "https://spec.edmcouncil.org/fibo/BE/LegalEntities/FormalBusinessOrganizations/">
	<!ENTITY fibo-be-le-lei "https://spec.edmcouncil.org/fibo/BE/LegalEntities/LEIEntities/">
	<!ENTITY fibo-be-le-lp "https://spec.edmcouncil.org/fibo/BE/LegalEntities/LegalPersons/">
	<!ENTITY fibo-be-oac-opty "https://spec.edmcouncil.org/fibo/BE/OwnershipAndControl/OwnershipParties/">
	<!ENTITY fibo-fbc-fct-rga "https://spec.edmcouncil.org/fibo/FBC/FunctionalEntities/RegulatoryAgencies/">
	<!ENTITY fibo-fbc-fi-fi "https://spec.edmcouncil.org/fibo/FBC/FinancialInstruments/FinancialInstruments/">
	<!ENTITY fibo-fbc-pas-caa "https://spec.edmcouncil.org/fibo/FBC/ProductsAndServices/ClientsAndAccounts/">
	<!ENTITY fibo-fbc-pas-fpas "https://spec.edmcouncil.org/fibo/FBC/ProductsAndServices/FinancialProductsAndServices/">
	<!ENTITY fibo-fnd-aap-agt "https://spec.edmcouncil.org/fibo/FND/AgentsAndPeople/Agents/">
	<!ENTITY fibo-fnd-aap-ppl "https://spec.edmcouncil.org/fibo/FND/AgentsAndPeople/People/">
	<!ENTITY fibo-fnd-acc-cur "https://spec.edmcouncil.org/fibo/FND/Accounting/CurrencyAmount/">
	<!ENTITY fibo-fnd-agr-agr "https://spec.edmcouncil.org/fibo/FND/Agreements/Agreements/">
	<!ENTITY fibo-fnd-agr-ctr "https://spec.edmcouncil.org/fibo/FND/Agreements/Contracts/">
	<!ENTITY fibo-fnd-arr-arr "https://spec.edmcouncil.org/fibo/FND/Arrangements/Arrangements/">
	<!ENTITY fibo-fnd-arr-cls "https://spec.edmcouncil.org/fibo/FND/Arrangements/ClassificationSchemes/">
	<!ENTITY fibo-fnd-arr-doc "https://spec.edmcouncil.org/fibo/FND/Arrangements/Documents/">
	<!ENTITY fibo-fnd-arr-id "https://spec.edmcouncil.org/fibo/FND/Arrangements/IdentifiersAndIndices/">
	<!ENTITY fibo-fnd-dt-fd "https://spec.edmcouncil.org/fibo/FND/DatesAndTimes/FinancialDates/">
	<!ENTITY fibo-fnd-dt-oc "https://spec.edmcouncil.org/fibo/FND/DatesAndTimes/Occurrences/">
	<!ENTITY fibo-fnd-oac-own "https://spec.edmcouncil.org/fibo/FND/OwnershipAndControl/Ownership/">
	<!ENTITY fibo-fnd-org-fm "https://spec.edmcouncil.org/fibo/FND/Organizations/FormalOrganizations/">
	<!ENTITY fibo-fnd-org-org "https://spec.edmcouncil.org/fibo/FND/Organizations/Organizations/">
	<!ENTITY fibo-fnd-pas-pas "https://spec.edmcouncil.org/fibo/FND/ProductsAndServices/ProductsAndServices/">
	<!ENTITY fibo-fnd-plc-adr "https://spec.edmcouncil.org/fibo/FND/Places/Addresses/">
	<!ENTITY fibo-fnd-plc-cr "https://spec.edmcouncil.org/fibo/FND/Places/CountryRepresentation/">
	<!ENTITY fibo-fnd-plc-cty "https://spec.edmcouncil.org/fibo/FND/Places/Countries/">
	<!ENTITY fibo-fnd-plc-loc "https://spec.edmcouncil.org/fibo/FND/Places/Locations/">
	<!ENTITY fibo-fnd-pty-pty "https://spec.edmcouncil.org/fibo/FND/Parties/Parties/">
	<!ENTITY fibo-fnd-qt-qtu "https://spec.edmcouncil.org/fibo/FND/Quantities/QuantitiesAndUnits/">
	<!ENTITY fibo-fnd-rel-rel "https://spec.edmcouncil.org/fibo/FND/Relations/Relations/">
	<!ENTITY fibo-fnd-utl-av "https://spec.edmcouncil.org/fibo/FND/Utilities/AnnotationVocabulary/">
	<!ENTITY fibo-fnd-utl-bt "https://spec.edmcouncil.org/fibo/FND/Utilities/BusinessFacingTypes/">
	<!ENTITY fibo-ln-ln-up "https://spec.edmcouncil.org/fibo/LOAN/LoanContracts/LoanUpperTemp/">
	<!ENTITY loan "https://spec.edmcouncil.org/fibo/LOAN/LoanContracts/LoanCore/">
	<!ENTITY owl "http://www.w3.org/2002/07/owl#">
	<!ENTITY rdf "http://www.w3.org/1999/02/22-rdf-syntax-ns#">
	<!ENTITY rdfs "http://www.w3.org/2000/01/rdf-schema#">
	<!ENTITY skos "http://www.w3.org/2004/02/skos/core#">
	<!ENTITY sm "http://www.omg.org/techprocess/ab/SpecificationMetadata/">
	<!ENTITY xs "http://www.w3.org/2001/XMLSchema#">
]>
<rdf:RDF
	xml:base="https://spec.edmcouncil.org/fibo/LOAN/LoanContracts/LoanUpperTemp/"
	xmlns:dct="http://purl.org/dc/terms/"
	xmlns:fibo-be-le-fbo="https://spec.edmcouncil.org/fibo/BE/LegalEntities/FormalBusinessOrganizations/"
	xmlns:fibo-be-le-lei="https://spec.edmcouncil.org/fibo/BE/LegalEntities/LEIEntities/"
	xmlns:fibo-be-le-lp="https://spec.edmcouncil.org/fibo/BE/LegalEntities/LegalPersons/"
	xmlns:fibo-be-oac-opty="https://spec.edmcouncil.org/fibo/BE/OwnershipAndControl/OwnershipParties/"
	xmlns:fibo-fbc-fct-rga="https://spec.edmcouncil.org/fibo/FBC/FunctionalEntities/RegulatoryAgencies/"
	xmlns:fibo-fbc-fi-fi="https://spec.edmcouncil.org/fibo/FBC/FinancialInstruments/FinancialInstruments/"
	xmlns:fibo-fbc-pas-caa="https://spec.edmcouncil.org/fibo/FBC/ProductsAndServices/ClientsAndAccounts/"
	xmlns:fibo-fbc-pas-fpas="https://spec.edmcouncil.org/fibo/FBC/ProductsAndServices/FinancialProductsAndServices/"
	xmlns:fibo-fnd-aap-agt="https://spec.edmcouncil.org/fibo/FND/AgentsAndPeople/Agents/"
	xmlns:fibo-fnd-aap-ppl="https://spec.edmcouncil.org/fibo/FND/AgentsAndPeople/People/"
	xmlns:fibo-fnd-acc-cur="https://spec.edmcouncil.org/fibo/FND/Accounting/CurrencyAmount/"
	xmlns:fibo-fnd-agr-agr="https://spec.edmcouncil.org/fibo/FND/Agreements/Agreements/"
	xmlns:fibo-fnd-agr-ctr="https://spec.edmcouncil.org/fibo/FND/Agreements/Contracts/"
	xmlns:fibo-fnd-arr-arr="https://spec.edmcouncil.org/fibo/FND/Arrangements/Arrangements/"
	xmlns:fibo-fnd-arr-cls="https://spec.edmcouncil.org/fibo/FND/Arrangements/ClassificationSchemes/"
	xmlns:fibo-fnd-arr-doc="https://spec.edmcouncil.org/fibo/FND/Arrangements/Documents/"
	xmlns:fibo-fnd-arr-id="https://spec.edmcouncil.org/fibo/FND/Arrangements/IdentifiersAndIndices/"
	xmlns:fibo-fnd-dt-fd="https://spec.edmcouncil.org/fibo/FND/DatesAndTimes/FinancialDates/"
	xmlns:fibo-fnd-dt-oc="https://spec.edmcouncil.org/fibo/FND/DatesAndTimes/Occurrences/"
	xmlns:fibo-fnd-oac-own="https://spec.edmcouncil.org/fibo/FND/OwnershipAndControl/Ownership/"
	xmlns:fibo-fnd-org-fm="https://spec.edmcouncil.org/fibo/FND/Organizations/FormalOrganizations/"
	xmlns:fibo-fnd-org-org="https://spec.edmcouncil.org/fibo/FND/Organizations/Organizations/"
	xmlns:fibo-fnd-pas-pas="https://spec.edmcouncil.org/fibo/FND/ProductsAndServices/ProductsAndServices/"
	xmlns:fibo-fnd-plc-adr="https://spec.edmcouncil.org/fibo/FND/Places/Addresses/"
	xmlns:fibo-fnd-plc-cr="https://spec.edmcouncil.org/fibo/FND/Places/CountryRepresentation/"
	xmlns:fibo-fnd-plc-cty="https://spec.edmcouncil.org/fibo/FND/Places/Countries/"
	xmlns:fibo-fnd-plc-loc="https://spec.edmcouncil.org/fibo/FND/Places/Locations/"
	xmlns:fibo-fnd-pty-pty="https://spec.edmcouncil.org/fibo/FND/Parties/Parties/"
	xmlns:fibo-fnd-qt-qtu="https://spec.edmcouncil.org/fibo/FND/Quantities/QuantitiesAndUnits/"
	xmlns:fibo-fnd-rel-rel="https://spec.edmcouncil.org/fibo/FND/Relations/Relations/"
	xmlns:fibo-fnd-utl-av="https://spec.edmcouncil.org/fibo/FND/Utilities/AnnotationVocabulary/"
	xmlns:fibo-fnd-utl-bt="https://spec.edmcouncil.org/fibo/FND/Utilities/BusinessFacingTypes/"
	xmlns:fibo-ln-ln-up="https://spec.edmcouncil.org/fibo/LOAN/LoanContracts/LoanUpperTemp/"
	xmlns:loan="https://spec.edmcouncil.org/fibo/LOAN/LoanContracts/LoanCore/"
	xmlns:owl="http://www.w3.org/2002/07/owl#"
	xmlns:rdf="http://www.w3.org/1999/02/22-rdf-syntax-ns#"
	xmlns:rdfs="http://www.w3.org/2000/01/rdf-schema#"
	xmlns:skos="http://www.w3.org/2004/02/skos/core#"
	xmlns:sm="http://www.omg.org/techprocess/ab/SpecificationMetadata/"
	xmlns:xs="http://www.w3.org/2001/XMLSchema#">
	
	<owl:Ontology
		rdf:about="https://spec.edmcouncil.org/fibo/LOAN/LoanContracts/LoanUpperTemp/">
		<owl:imports
			rdf:resource="https://spec.edmcouncil.org/fibo/FND/DatesAndTimes/FinancialDates/"/>
		<owl:versionInfo>Created with e6Tools Graphical OWL Editor from D:\SEMANTIC-ARTS\NAS\ClientsAndPartners\EDM Council\fibo ontologies\LoanOntology\loans.vsdx Page:loanUpper</owl:versionInfo>
		<skos:definition></skos:definition>
		<skos:definition>LoanUpperTemp</skos:definition>
	</owl:Ontology>
	
	<owl:AnnotationProperty
		rdf:about="&sm;normativeReference">
	</owl:AnnotationProperty>
	
	<owl:ObjectProperty
		rdf:about="&skos;broaderTransitive">
	</owl:ObjectProperty>
	
	<owl:AnnotationProperty
		rdf:about="&skos;definition">
	</owl:AnnotationProperty>
	
	<owl:AnnotationProperty
		rdf:about="&skos;editorialNote">
	</owl:AnnotationProperty>
	
	<owl:ObjectProperty
		rdf:about="&fibo-be-oac-opty;guarantees">
		<owl:inverseOf
			rdf:resource="&fibo-ln-ln-up;opty-isGuaranteedBy"/>
		<skos:editorialNote>Adding inverse of guarantees called isGuaranteedBy</skos:editorialNote>
		<skos:editorialNote>Topic: BE add inverse of guarantees called isGuaranteedBy</skos:editorialNote>
	</owl:ObjectProperty>
	
	<owl:Class
		rdf:about="&fibo-fnd-acc-cur;MonetaryAmount">
	</owl:Class>
	
	<owl:Class
		rdf:about="&fibo-fnd-aap-agt;AutonomousAgent">
	</owl:Class>
	
	<owl:Class
		rdf:about="&fibo-fnd-aap-ppl;LegallyCapablePerson">
	</owl:Class>
	
	<owl:Class
		rdf:about="&fibo-fnd-agr-agr;Agreement">
		<rdfs:subClassOf
			rdf:resource="&fibo-ln-ln-up;Specification"/>
	</owl:Class>
	
	<owl:Class
		rdf:about="&fibo-fnd-agr-agr;Commitment">
		<rdfs:subClassOf
			rdf:resource="&fibo-ln-ln-up;Specification"/>
		<rdfs:subClassOf>
			<owl:Restriction>
				<owl:onProperty
					rdf:resource="&fibo-ln-ln-up;hasPartyWithDuty"/>
				<owl:someValuesFrom
					rdf:resource="&fibo-fnd-pty-pty;IndependentParty"/>
			</owl:Restriction>
		</rdfs:subClassOf>
		<rdfs:subClassOf>
			<owl:Restriction>
				<owl:onProperty
					rdf:resource="&fibo-ln-ln-up;hasPartyWithRight"/>
				<owl:someValuesFrom
					rdf:resource="&fibo-fnd-pty-pty;IndependentParty"/>
			</owl:Restriction>
		</rdfs:subClassOf>
	</owl:Class>
	
	<owl:ObjectProperty
		rdf:about="&fibo-fnd-agr-ctr;hasEffectiveDate">
		<rdfs:subPropertyOf
			rdf:resource="&fibo-ln-ln-up;asOfDate"/>
	</owl:ObjectProperty>
	
	<owl:Class
		rdf:about="&fibo-fnd-arr-arr;Collection">
	</owl:Class>
	
	<owl:Class
		rdf:about="&fibo-fnd-arr-cls;Classifier">
	</owl:Class>
	
	<owl:Class
		rdf:about="&fibo-fnd-dt-fd;DatePeriod">
	</owl:Class>
	
	<owl:Class
		rdf:about="&fibo-fnd-dt-fd;Schedule">
	</owl:Class>
	
	<owl:DatatypeProperty
		rdf:about="&fibo-fnd-dt-fd;hasCount">
	</owl:DatatypeProperty>
	
	<owl:ObjectProperty
		rdf:about="&fibo-fnd-dt-fd;hasDate">
	</owl:ObjectProperty>
	
	<owl:ObjectProperty
		rdf:about="&fibo-fnd-dt-fd;hasDatePeriod">
	</owl:ObjectProperty>
	
	<owl:ObjectProperty
		rdf:about="&fibo-fnd-dt-fd;hasStartDate">
	</owl:ObjectProperty>
	
	<owl:Class
		rdf:about="&fibo-fnd-dt-oc;Occurrence">
	</owl:Class>
	
	<owl:Class
		rdf:about="&fibo-fnd-pty-pty;IndependentParty">
	</owl:Class>
	
	<owl:Class
		rdf:about="&fibo-fnd-plc-adr;VirtualAddress">
	</owl:Class>
	
	<owl:Class
		rdf:about="&fibo-fnd-plc-cty;GeopoliticalEntity">
	</owl:Class>
	
	<owl:ObjectProperty
		rdf:about="&fibo-fnd-plc-cr;isSubdivisionOf">
	</owl:ObjectProperty>
	
	<owl:Class
		rdf:about="&fibo-fnd-pas-pas;Product">
	</owl:Class>
	
	<owl:ObjectProperty
		rdf:about="&fibo-fnd-rel-rel;Classifies">
	</owl:ObjectProperty>
	
	<owl:ObjectProperty
		rdf:about="&fibo-fnd-rel-rel;comprises">
	</owl:ObjectProperty>
	
	<owl:ObjectProperty
		rdf:about="&fibo-fnd-rel-rel;has">
	</owl:ObjectProperty>
	
	<owl:ObjectProperty
		rdf:about="&fibo-fnd-rel-rel;hasMember">
	</owl:ObjectProperty>
	
	<owl:ObjectProperty
		rdf:about="&fibo-fnd-rel-rel;isClassifiedBy">
	</owl:ObjectProperty>
	
	<owl:AnnotationProperty
		rdf:about="&fibo-fnd-utl-av;explanatoryNote">
	</owl:AnnotationProperty>
	
	<owl:AnnotationProperty
		rdf:about="&fibo-fnd-utl-av;usageNote">
	</owl:AnnotationProperty>
	
	<owl:Class
		rdf:about="https://spec.edmcouncil.org/fibo/LOAN/LoanContracts/LoanUpperTemp/#fibo-fnd-rel-relClassifies_some_fibo-fnd-aap-pplPerson">
		<rdfs:subClassOf
			rdf:resource="&fibo-ln-ln-up;Ethnicity"/>
		<rdfs:subClassOf
			rdf:resource="&fibo-ln-ln-up;Race"/>
		<owl:equivalentClass>
			<owl:Restriction>
				<owl:onProperty
					rdf:resource="&fibo-fnd-rel-rel;Classifies"/>
				<owl:someValuesFrom
					rdf:resource="&fibo-fnd-aap-ppl;Person"/>
			</owl:Restriction>
		</owl:equivalentClass>
	</owl:Class>
	
	<owl:Class
		rdf:about="https://spec.edmcouncil.org/fibo/LOAN/LoanContracts/LoanUpperTemp/#skosbroaderTransitive_some_fibo-ln-ln-upEthnicity">
		<rdfs:subClassOf
			rdf:resource="&fibo-ln-ln-up;Ethnicity"/>
		<owl:equivalentClass>
			<owl:Restriction>
				<owl:onProperty
					rdf:resource="&skos;broaderTransitive"/>
				<owl:someValuesFrom
					rdf:resource="&fibo-ln-ln-up;Ethnicity"/>
			</owl:Restriction>
		</owl:equivalentClass>
	</owl:Class>
	
	<owl:Class
		rdf:about="https://spec.edmcouncil.org/fibo/LOAN/LoanContracts/LoanUpperTemp/#skosbroaderTransitive_some_fibo-ln-ln-upRace">
		<rdfs:subClassOf
			rdf:resource="&fibo-ln-ln-up;Race"/>
		<owl:equivalentClass>
			<owl:Restriction>
				<owl:onProperty
					rdf:resource="&skos;broaderTransitive"/>
				<owl:someValuesFrom
					rdf:resource="&fibo-ln-ln-up;Race"/>
			</owl:Restriction>
		</owl:equivalentClass>
	</owl:Class>
	
	<owl:Class
		rdf:about="&fibo-ln-ln-up;ActualPayment">
		<rdfs:subClassOf
			rdf:resource="&fibo-fnd-dt-oc;Occurrence"/>
		<rdfs:subClassOf>
			<owl:Restriction>
				<owl:onProperty
					rdf:resource="&fibo-fnd-dt-fd;hasDate"/>
				<owl:someValuesFrom
					rdf:resource="&fibo-fnd-dt-fd;Date"/>
			</owl:Restriction>
		</rdfs:subClassOf>
		<rdfs:subClassOf>
			<owl:Restriction>
				<owl:onProperty
					rdf:resource="&fibo-ln-ln-up;cur-hasAmount"/>
				<owl:someValuesFrom
					rdf:resource="&fibo-fnd-acc-cur;MonetaryAmount"/>
			</owl:Restriction>
		</rdfs:subClassOf>
		<skos:definition>An actual payment occcurrence, whereby the borrower submits payment in order to fulfill an obligation to repay a loan.</skos:definition>
		<skos:editorialNote>Topic: Payments</skos:editorialNote>
	</owl:Class>
	
	<owl:Class
		rdf:about="&fibo-ln-ln-up;Application">
		<rdfs:subClassOf
			rdf:resource="&fibo-ln-ln-up;fnd-Request"/>
		<rdfs:subClassOf>
			<owl:Restriction>
				<owl:onProperty
					rdf:resource="&fibo-ln-ln-up;hasDateReceived"/>
				<owl:someValuesFrom
					rdf:resource="&fibo-fnd-dt-fd;Date"/>
			</owl:Restriction>
		</rdfs:subClassOf>
		<skos:definition>A request submitted by an applicant to receive something (e.g. a licence, a loan, a membership).  Is accompanied by documentation of pertinent information to determine whether the request should be granted.</skos:definition>
	</owl:Class>
	
	<owl:Class
		rdf:about="&fibo-ln-ln-up;BE-ContactPurpose">
		<rdfs:subClassOf
			rdf:resource="&fibo-fnd-arr-cls;Classifier"/>
		<skos:definition>A virtual address for communication via phone.</skos:definition>
	</owl:Class>
	
	<owl:Class
		rdf:about="&fibo-ln-ln-up;ChargeCategory">
		<rdfs:subClassOf
			rdf:resource="&fibo-fnd-arr-cls;Classifier"/>
		<skos:definition>A specific indicator of what a charge is for (e.g. closing costs, interest)</skos:definition>
	</owl:Class>
	
	<owl:Class
		rdf:about="&fibo-ln-ln-up;ConstructionType">
		<rdfs:subClassOf
			rdf:resource="&fibo-fnd-arr-cls;Classifier"/>
		<skos:definition>A particular kind of construction</skos:definition>
		<skos:editorialNote>Topic: RealEstate</skos:editorialNote>
	</owl:Class>
	
	<owl:Class
		rdf:about="&fibo-ln-ln-up;ContactInfo">
		<rdfs:subClassOf>
			<owl:Restriction>
				<owl:minQualifiedCardinality
					rdf:datatype="&xs;nonNegativeInteger">0</owl:minQualifiedCardinality>
				<owl:onClass
					rdf:resource="&fibo-fnd-aap-ppl;LegallyCapableAdult"/>
				<owl:onProperty
					rdf:resource="&fibo-fnd-rel-rel;comprises"/>
			</owl:Restriction>
		</rdfs:subClassOf>
		<rdfs:subClassOf>
			<owl:Restriction>
				<owl:minQualifiedCardinality
					rdf:datatype="&xs;nonNegativeInteger">0</owl:minQualifiedCardinality>
				<owl:onClass
					rdf:resource="&fibo-fnd-org-fm;FormalOrganization"/>
				<owl:onProperty
					rdf:resource="&fibo-fnd-rel-rel;comprises"/>
			</owl:Restriction>
		</rdfs:subClassOf>
		<rdfs:subClassOf>
			<owl:Restriction>
				<owl:minQualifiedCardinality
					rdf:datatype="&xs;nonNegativeInteger">0</owl:minQualifiedCardinality>
				<owl:onClass
					rdf:resource="&fibo-fnd-plc-adr;PostalAddress"/>
				<owl:onProperty
					rdf:resource="&fibo-fnd-rel-rel;comprises"/>
			</owl:Restriction>
		</rdfs:subClassOf>
		<rdfs:subClassOf>
			<owl:Restriction>
				<owl:minQualifiedCardinality
					rdf:datatype="&xs;nonNegativeInteger">0</owl:minQualifiedCardinality>
				<owl:onClass
					rdf:resource="&fibo-ln-ln-up;adr-EmailAddress"/>
				<owl:onProperty
					rdf:resource="&fibo-fnd-rel-rel;comprises"/>
			</owl:Restriction>
		</rdfs:subClassOf>
		<rdfs:subClassOf>
			<owl:Restriction>
				<owl:minQualifiedCardinality
					rdf:datatype="&xs;nonNegativeInteger">0</owl:minQualifiedCardinality>
				<owl:onClass
					rdf:resource="&fibo-ln-ln-up;adr-PhoneNumber"/>
				<owl:onProperty
					rdf:resource="&fibo-fnd-rel-rel;comprises"/>
			</owl:Restriction>
		</rdfs:subClassOf>
		<rdfs:subClassOf>
			<owl:Restriction>
				<owl:onProperty
					rdf:resource="&fibo-fnd-rel-rel;isClassifiedBy"/>
				<owl:someValuesFrom
					rdf:resource="&fibo-ln-ln-up;BE-ContactPurpose"/>
			</owl:Restriction>
		</rdfs:subClassOf>
		<skos:definition>A way to make contact with a person or organization for a particular reason regarding something.  The details may be role-specific, so the information cannot always go on the individual or organization.</skos:definition>
		<skos:editorialNote>This approach avoids the need to have multiple properties to connect different things to ContactInfo use for different purposes.</skos:editorialNote>
		<skos:editorialNote>Topic: BE</skos:editorialNote>
		<fibo-fnd-utl-av:usageNote>Make sure to check the existing instances of ContactPurpose and use those before creating new ones.</fibo-fnd-utl-av:usageNote>
	</owl:Class>
	
	<owl:Class
		rdf:about="&fibo-ln-ln-up;DwellingCapacity">
		<rdfs:subClassOf
			rdf:resource="&fibo-fnd-arr-cls;Classifier"/>
		<skos:definition>A category indicating how many dwellings some property has.</skos:definition>
		<skos:editorialNote>Topic: RealEstate</skos:editorialNote>
	</owl:Class>
	
	<owl:Class
		rdf:about="&fibo-ln-ln-up;Ethnicity">
		<rdfs:subClassOf
			rdf:resource="&fibo-fnd-arr-cls;Classifier"/>
		<skos:definition>A category based on a cultural factors, including nationality, regional culture, ancestry, and language</skos:definition>
	</owl:Class>
	
	<owl:Class
		rdf:about="&fibo-ln-ln-up;FND-InformationProduct">
		<rdfs:subClassOf
			rdf:resource="&fibo-fnd-pas-pas;Product"/>
		<skos:definition>A Product that is informational in nature, rather than physical.</skos:definition>
	</owl:Class>
	
	<owl:Class
		rdf:about="&fibo-ln-ln-up;MetroDivision">
		<rdfs:subClassOf
			rdf:resource="&fibo-fnd-plc-cty;GeopoliticalEntity"/>
		<rdfs:subClassOf>
			<owl:Restriction>
				<owl:onProperty
					rdf:resource="&fibo-fnd-plc-cr;isSubdivisionOf"/>
				<owl:someValuesFrom
					rdf:resource="&fibo-ln-ln-up;MetroStatArea"/>
			</owl:Restriction>
		</rdfs:subClassOf>
		<skos:definition>Metropolitan division (MD) is an area specified by the government to describe a subsection of a certain metropolitan statistical area.  In the US, this is governed by the Census Department.</skos:definition>
		<skos:editorialNote>Topic: Regions</skos:editorialNote>
	</owl:Class>
	
	<owl:Class
		rdf:about="&fibo-ln-ln-up;MetroStatArea">
		<rdfs:subClassOf
			rdf:resource="&fibo-fnd-plc-cty;GeopoliticalEntity"/>
		<skos:definition>Metropolitan statistical area (MSA) is an area specified by the government to describe a certain metropolitan statistical area.  In the US, this is governed by the Census department.</skos:definition>
		<skos:editorialNote>Topic: Regions</skos:editorialNote>
	</owl:Class>
	
	<owl:Class
		rdf:about="&fibo-ln-ln-up;PaymentHistory">
		<rdfs:subClassOf
			rdf:resource="&fibo-ln-ln-up;TransactionHistory"/>
		<rdfs:subClassOf>
			<owl:Restriction>
				<owl:onProperty
					rdf:resource="&fibo-fnd-rel-rel;hasMember"/>
				<owl:someValuesFrom
					rdf:resource="&fibo-ln-ln-up;ActualPayment"/>
			</owl:Restriction>
		</rdfs:subClassOf>
		<rdfs:subClassOf>
			<owl:Restriction>
				<owl:onProperty
					rdf:resource="&fibo-ln-ln-up;hasActualUnpaidBalance"/>
				<owl:someValuesFrom
					rdf:resource="&fibo-fnd-acc-cur;MonetaryAmount"/>
			</owl:Restriction>
		</rdfs:subClassOf>
		<skos:definition>A record of actual payments of principal, interest, and other related amounts made by a borrower to a lender or servicer in order to fulfill their re-payment obligation.</skos:definition>
		<skos:editorialNote>Topic: Payments</skos:editorialNote>
		<fibo-fnd-utl-av:explanatoryNote>Just like a PaymentSchedule except that the dates and amounts are actuals.</fibo-fnd-utl-av:explanatoryNote>
	</owl:Class>
	
	<owl:Class
		rdf:about="&fibo-ln-ln-up;PaymentSchedule">
		<rdfs:subClassOf
			rdf:resource="&fibo-fnd-arr-arr;Collection"/>
		<rdfs:subClassOf
			rdf:resource="&fibo-fnd-dt-fd;Schedule"/>
		<rdfs:subClassOf>
			<owl:Restriction>
				<owl:onProperty
					rdf:resource="&fibo-fnd-rel-rel;hasMember"/>
				<owl:someValuesFrom
					rdf:resource="&fibo-ln-ln-up;ScheduledPayment"/>
			</owl:Restriction>
		</rdfs:subClassOf>
		<rdfs:subClassOf>
			<owl:Restriction>
				<owl:onProperty
					rdf:resource="&fibo-ln-ln-up;hasScheduledUnpaidBalance"/>
				<owl:someValuesFrom
					rdf:resource="&fibo-fnd-acc-cur;MonetaryAmount"/>
			</owl:Restriction>
		</rdfs:subClassOf>
		<skos:definition>A Schedule of amounts of principal and interest that are due over the term of the loan in order to fully pay off the obligation.</skos:definition>
		<skos:editorialNote>Topic: Payments</skos:editorialNote>
	</owl:Class>
	
	<owl:Class
		rdf:about="&fibo-ln-ln-up;PropertyInspection">
		<rdfs:subClassOf
			rdf:resource="&fibo-fnd-dt-oc;Occurrence"/>
		<rdfs:subClassOf>
			<owl:Restriction>
				<owl:minQualifiedCardinality
					rdf:datatype="&xs;nonNegativeInteger">1</owl:minQualifiedCardinality>
				<owl:onClass
					rdf:resource="&fibo-fnd-plc-loc;RealEstate"/>
				<owl:onProperty
					rdf:resource="&fibo-ln-ln-up;hasItemInspected"/>
			</owl:Restriction>
		</rdfs:subClassOf>
		<rdfs:subClassOf>
			<owl:Restriction>
				<owl:onProperty
					rdf:resource="&fibo-ln-ln-up;performedBy"/>
				<owl:someValuesFrom
					rdf:resource="&fibo-fnd-pty-pty;IndependentParty"/>
			</owl:Restriction>
		</rdfs:subClassOf>
		<skos:definition>The act of analyzing one or more aspects of a real property for independent assessment of status or deficiency.</skos:definition>
		<fibo-fnd-utl-av:explanatoryNote>This is independent and separate from conducting an appraisal. Examples are termite inspections, construction inspections, etc.</fibo-fnd-utl-av:explanatoryNote>
	</owl:Class>
	
	<owl:Class
		rdf:about="&fibo-ln-ln-up;Race">
		<rdfs:subClassOf
			rdf:resource="&fibo-fnd-arr-cls;Classifier"/>
		<skos:definition>A category based on a person&apos;s physical characteristics, such as bone structure and skin, hair, or eye color.</skos:definition>
	</owl:Class>
	
	<owl:Class
		rdf:about="&fibo-ln-ln-up;Report">
		<rdfs:subClassOf>
			<owl:Restriction>
				<owl:minQualifiedCardinality
					rdf:datatype="&xs;nonNegativeInteger">0</owl:minQualifiedCardinality>
				<owl:onClass
					rdf:resource="&fibo-fnd-aap-agt;AutonomousAgent"/>
				<owl:onProperty
					rdf:resource="&fibo-ln-ln-up;rel-isProducedBy_I"/>
			</owl:Restriction>
		</rdfs:subClassOf>
		<rdfs:subClassOf>
			<owl:Restriction>
				<owl:minQualifiedCardinality
					rdf:datatype="&xs;nonNegativeInteger">0</owl:minQualifiedCardinality>
				<owl:onClass
					rdf:resource="&fibo-fnd-dt-fd;DatePeriod"/>
				<owl:onProperty
					rdf:resource="&fibo-ln-ln-up;dt-fd-coversPeriod"/>
			</owl:Restriction>
		</rdfs:subClassOf>
		<rdfs:subClassOf>
			<owl:Restriction>
				<owl:onProperty
					rdf:resource="&fibo-ln-ln-up;hasCreationDate"/>
				<owl:someValuesFrom
					rdf:resource="&fibo-fnd-dt-fd;Date"/>
			</owl:Restriction>
		</rdfs:subClassOf>
		<sm:normativeReference>http://www.businessdictionary.com/definition/report.html</sm:normativeReference>
		<skos:definition>A body of information organized in a narrative, graphic, or tabular form, prepared on ad hoc, periodic, recurring, regular, or as required basis. Reports may refer to specific periods, events, occurrences, or subjects, and may be communicated or presented in oral or written form.</skos:definition>
	</owl:Class>
	
	<owl:Class
		rdf:about="&fibo-ln-ln-up;RiskAssesssment">
		<rdfs:subClassOf
			rdf:resource="&fibo-fnd-dt-oc;Occurrence"/>
		<skos:definition>An information product derived from the transaction history of a credit account.</skos:definition>
	</owl:Class>
	
	<owl:Class
		rdf:about="&fibo-ln-ln-up;ScheduledPayment">
		<rdfs:subClassOf
			rdf:resource="&fibo-fnd-agr-agr;Commitment"/>
		<rdfs:subClassOf>
			<owl:Restriction>
				<owl:onProperty
					rdf:resource="&fibo-fnd-dt-fd;hasDate"/>
				<owl:someValuesFrom
					rdf:resource="&fibo-fnd-dt-fd;Date"/>
			</owl:Restriction>
		</rdfs:subClassOf>
		<rdfs:subClassOf>
			<owl:Restriction>
				<owl:onProperty
					rdf:resource="&fibo-ln-ln-up;cur-hasAmount"/>
				<owl:someValuesFrom
					rdf:resource="&fibo-fnd-acc-cur;MonetaryAmount"/>
			</owl:Restriction>
		</rdfs:subClassOf>
		<skos:definition>A scheduled payment occurrence that is part of a payment schedule covering the term of the loan.</skos:definition>
		<skos:editorialNote>Topic: Payments</skos:editorialNote>
	</owl:Class>
	
	<owl:Class
		rdf:about="&fibo-ln-ln-up;Specification">
		<skos:definition>A body of information specifying what properties, structure and/or results something should or must have after it has been built, fulfilled or completed. The thing may be physical (a building), organizational (a management structure), computational (a program), job or task related (e.g., a CEO, Chief Judge) or changing oil in a car. It may be a set of characteristics saying what something must be, or a set of instructions saying how to do something.</skos:definition>
	</owl:Class>
	
	<owl:Class
		rdf:about="&fibo-ln-ln-up;Text">
		<rdfs:subClassOf>
			<owl:Restriction>
				<owl:onProperty
					rdf:resource="&fibo-ln-ln-up;hasString"/>
				<owl:someValuesFrom
					rdf:resource="&xs;string"/>
			</owl:Restriction>
		</rdfs:subClassOf>
		<skos:definition>A set of words and characters expressed in some language. E.g. a description, a message</skos:definition>
		<skos:editorialNote>This probably belongs in a documents messages ontology</skos:editorialNote>
	</owl:Class>
	
	<owl:Class
		rdf:about="&fibo-ln-ln-up;TransactionEvent">
		<rdfs:subClassOf
			rdf:resource="&fibo-fnd-dt-oc;Occurrence"/>
		<skos:definition></skos:definition>
		<skos:editorialNote>This is a more appropriate version of  fibo-fnd-pas-pas:TransactionEvent which is wrongly a subclass of OccurenceKind</skos:editorialNote>
		<skos:editorialNote>Topic: Accounts</skos:editorialNote>
	</owl:Class>
	
	<owl:Class
		rdf:about="&fibo-ln-ln-up;TransactionHistory">
		<rdfs:subClassOf
			rdf:resource="&fibo-fnd-arr-arr;Collection"/>
		<rdfs:subClassOf>
			<owl:Restriction>
				<owl:onProperty
					rdf:resource="&fibo-fnd-rel-rel;hasMember"/>
				<owl:someValuesFrom
					rdf:resource="&fibo-ln-ln-up;TransactionEvent"/>
			</owl:Restriction>
		</rdfs:subClassOf>
		<rdfs:subClassOf>
			<owl:Restriction>
				<owl:onProperty
					rdf:resource="&fibo-ln-ln-up;rel-isOf"/>
				<owl:someValuesFrom
					rdf:resource="&fibo-fnd-agr-ctr;Contract"/>
			</owl:Restriction>
		</rdfs:subClassOf>
		<skos:definition>A record of actual account transactions, be they payments, withdrawls etc.</skos:definition>
		<skos:editorialNote>Topic: Accounts and Transactions</skos:editorialNote>
	</owl:Class>
	
	<owl:Class
		rdf:about="&fibo-ln-ln-up;Valuation">
		<rdfs:subClassOf
			rdf:resource="&fibo-ln-ln-up;alx-Measurement"/>
		<rdfs:subClassOf>
			<owl:Restriction>
				<owl:minQualifiedCardinality
					rdf:datatype="&xs;nonNegativeInteger">1</owl:minQualifiedCardinality>
				<owl:onClass
					rdf:resource="&owl;Thing"/>
				<owl:onProperty
					rdf:resource="&fibo-ln-ln-up;thingBeingValued"/>
			</owl:Restriction>
		</rdfs:subClassOf>
		<skos:definition>A Measurement to assess the value of something, e.g. a house, or a bond. The result is in some currency.</skos:definition>
		<fibo-fnd-utl-av:explanatoryNote>TODO: model this out properly, add to analytics (alx) ontology, put it somewhere (in FBC?).</fibo-fnd-utl-av:explanatoryNote>
	</owl:Class>
	
	<fibo-ln-ln-up:ConstructionType
		rdf:about="&fibo-ln-ln-up;_manufactured">
		<rdf:type
			rdf:resource="&owl;Thing"/>
		<skos:definition>A factory built dwelling built in compliance with the Federal Manufactured Home Construction and Safety Standards in effect at the time the home was manufactured as evidenced by the HUD label.</skos:definition>
	</fibo-ln-ln-up:ConstructionType>
	
	<fibo-ln-ln-up:ConstructionType
		rdf:about="&fibo-ln-ln-up;_mobileHome">
		<rdf:type
			rdf:resource="&owl;Thing"/>
		<skos:definition>Dwelling unit constructed on a base frame which features wheels and axles to be used in transporting home from place to place, does not meet HUD code.</skos:definition>
	</fibo-ln-ln-up:ConstructionType>
	
	<fibo-ln-ln-up:ConstructionType
		rdf:about="&fibo-ln-ln-up;_modular">
		<rdf:type
			rdf:resource="&owl;Thing"/>
		<skos:definition>A factory built dwelling not on a permanent chassis.</skos:definition>
	</fibo-ln-ln-up:ConstructionType>
	
	<fibo-ln-ln-up:DwellingCapacity
		rdf:about="&fibo-ln-ln-up;_multiFamily">
		<rdf:type
			rdf:resource="&owl;Thing"/>
		<skos:definition>5 or more units</skos:definition>
	</fibo-ln-ln-up:DwellingCapacity>
	
	<fibo-ln-ln-up:ConstructionType
		rdf:about="&fibo-ln-ln-up;_onFrameModular">
		<rdf:type
			rdf:resource="&owl;Thing"/>
		<skos:definition>A factory built dwelling on a permanent chassis which does not have a HUD label.</skos:definition>
	</fibo-ln-ln-up:ConstructionType>
	
	<fibo-ln-ln-up:DwellingCapacity
		rdf:about="&fibo-ln-ln-up;_singleFamily">
		<rdf:type
			rdf:resource="&owl;Thing"/>
		<skos:definition>1-4 units</skos:definition>
	</fibo-ln-ln-up:DwellingCapacity>
	
	<fibo-ln-ln-up:ConstructionType
		rdf:about="&fibo-ln-ln-up;_siteBuilt">
		<rdf:type
			rdf:resource="&owl;Thing"/>
		<skos:definition>Describes construction process, indicating that most elements are created at the homes permanent site. May include some prefabricated components.</skos:definition>
	</fibo-ln-ln-up:ConstructionType>
	
	<owl:Class
		rdf:about="&fibo-ln-ln-up;adr-EmailAddress">
		<rdfs:subClassOf
			rdf:resource="&fibo-fnd-plc-adr;VirtualAddress"/>
		<rdfs:subClassOf>
			<owl:Restriction>
				<owl:onProperty
					rdf:resource="&fibo-ln-ln-up;hasString"/>
				<owl:someValuesFrom
					rdf:resource="&xs;string"/>
			</owl:Restriction>
		</rdfs:subClassOf>
		<skos:definition>A virtual address for sending email communication to.</skos:definition>
	</owl:Class>
	
	<owl:Class
		rdf:about="&fibo-ln-ln-up;adr-PhoneNumber">
		<rdfs:subClassOf
			rdf:resource="&fibo-fnd-plc-adr;VirtualAddress"/>
		<rdfs:subClassOf>
			<owl:Restriction>
				<owl:onProperty
					rdf:resource="&fibo-ln-ln-up;hasString"/>
				<owl:someValuesFrom
					rdf:resource="&xs;string"/>
			</owl:Restriction>
		</rdfs:subClassOf>
		<skos:definition>A virtual address for communication via phone.</skos:definition>
	</owl:Class>
	
	<owl:Class
		rdf:about="&fibo-ln-ln-up;alx-Measurement">
		<rdfs:subClassOf
			rdf:resource="&fibo-fnd-dt-oc;Occurrence"/>
		<skos:definition>The act of taking a measurement.  Some measurement procedure is used to measure some aspect of something giving a result typicalliy expressed in some units .  E.g. a valuation measuring the value of an asset expressedin USD</skos:definition>
		<fibo-fnd-utl-av:explanatoryNote>TODO: model this out properly, add to analytics (alx) ontology.</fibo-fnd-utl-av:explanatoryNote>
	</owl:Class>
	
	<owl:ObjectProperty
		rdf:about="&fibo-ln-ln-up;asOfDate">
		<rdfs:subPropertyOf
			rdf:resource="&fibo-fnd-dt-fd;hasDate"/>
		<skos:definition>LC to check: relates something to the date on which it is accurate or valid. E.g. a credit report has an asOfDate that means the date when the information was drawn. It is different from the creation date and need not be the last date of the DatePeriod covered.</skos:definition>
	</owl:ObjectProperty>
	
	<owl:ObjectProperty
		rdf:about="&fibo-ln-ln-up;conformsTo">
		<rdfs:range
			rdf:resource="&fibo-ln-ln-up;Specification"/>
		<skos:definition>The Subject  complies with or conforms to what is specified by the Object.  Often the Object  will causally affect the Subject, but not necessarily, hence is not a subproperty of fibo-fnd-rel-rel:causes</skos:definition>
	</owl:ObjectProperty>
	
	<owl:ObjectProperty
		rdf:about="&fibo-ln-ln-up;cur-hasAmount">
		<rdfs:subPropertyOf
			rdf:resource="&fibo-fnd-rel-rel;has"/>
		<rdfs:range
			rdf:resource="&fibo-fnd-acc-cur;MonetaryAmount"/>
		<skos:definition>Relates something to a monetary amount, e.g. credit limit, notional amount.</skos:definition>
		<fibo-fnd-utl-av:explanatoryNote>NOTE: this could be a loan amount, or a credit line. YES, we need to discuss; it could be even more that this.</fibo-fnd-utl-av:explanatoryNote>
	</owl:ObjectProperty>
	
	<owl:ObjectProperty
		rdf:about="&fibo-ln-ln-up;dataSourcedFrom">
		<skos:definition>A source of data, in a given context. e.g. Experian provides data for a CreditReport</skos:definition>
	</owl:ObjectProperty>
	
	<owl:ObjectProperty
		rdf:about="&fibo-ln-ln-up;dt-fd-coversPeriod">
		<rdfs:subPropertyOf
			rdf:resource="&fibo-fnd-dt-fd;hasDatePeriod"/>
		<rdfs:range
			rdf:resource="&fibo-fnd-dt-fd;DatePeriod"/>
		<skos:definition>The period of time which is covered. e.g. for a reporting period.</skos:definition>
	</owl:ObjectProperty>
	
	<owl:Class
		rdf:about="&fibo-ln-ln-up;fnd-Request">
		<rdfs:subClassOf
			rdf:resource="&fibo-fnd-dt-oc;Occurrence"/>
		<rdfs:subClassOf>
			<owl:Restriction>
				<owl:minQualifiedCardinality
					rdf:datatype="&xs;nonNegativeInteger">1</owl:minQualifiedCardinality>
				<owl:onClass
					rdf:resource="&owl;Thing"/>
				<owl:onProperty
					rdf:resource="&fibo-ln-ln-up;fnd-thingRequested"/>
			</owl:Restriction>
		</rdfs:subClassOf>
		<rdfs:subClassOf>
			<owl:Restriction>
				<owl:onProperty
					rdf:resource="&fibo-ln-ln-up;rel-from"/>
				<owl:someValuesFrom
					rdf:resource="&fibo-fnd-aap-agt;AutonomousAgent"/>
			</owl:Restriction>
		</rdfs:subClassOf>
		<rdfs:subClassOf>
			<owl:Restriction>
				<owl:onProperty
					rdf:resource="&fibo-ln-ln-up;rel-to"/>
				<owl:someValuesFrom
					rdf:resource="&fibo-fnd-aap-agt;AutonomousAgent"/>
			</owl:Restriction>
		</rdfs:subClassOf>
		<skos:definition>An agent asks another agent for something or to do something.</skos:definition>
	</owl:Class>
	
	<owl:Class
		rdf:about="&fibo-ln-ln-up;fnd-Response">
		<rdfs:subClassOf
			rdf:resource="&fibo-fnd-dt-oc;Occurrence"/>
		<rdfs:subClassOf>
			<owl:Restriction>
				<owl:minQualifiedCardinality
					rdf:datatype="&xs;nonNegativeInteger">1</owl:minQualifiedCardinality>
				<owl:onClass
					rdf:resource="&fibo-fnd-dt-oc;Occurrence"/>
				<owl:onProperty
					rdf:resource="&fibo-ln-ln-up;fnd-rel-isResponseTo"/>
			</owl:Restriction>
		</rdfs:subClassOf>
		<rdfs:subClassOf>
			<owl:Restriction>
				<owl:onProperty
					rdf:resource="&fibo-ln-ln-up;rel-from"/>
				<owl:someValuesFrom
					rdf:resource="&fibo-fnd-aap-agt;AutonomousAgent"/>
			</owl:Restriction>
		</rdfs:subClassOf>
		<rdfs:subClassOf>
			<owl:Restriction>
				<owl:onProperty
					rdf:resource="&fibo-ln-ln-up;rel-to"/>
				<owl:someValuesFrom
					rdf:resource="&fibo-fnd-aap-agt;AutonomousAgent"/>
			</owl:Restriction>
		</rdfs:subClassOf>
		<skos:definition>The act of responding to an Occurrence, often a communication.</skos:definition>
	</owl:Class>
	
	<owl:Class
		rdf:about="&fibo-ln-ln-up;fnd-RiskAssesssment">
		<rdfs:subClassOf
			rdf:resource="&fibo-fnd-dt-oc;Occurrence"/>
		<skos:definition>The occurrence of assessing the risk of something.</skos:definition>
	</owl:Class>
	
	<owl:ObjectProperty
		rdf:about="&fibo-ln-ln-up;fnd-rel-isResponseTo">
		<rdfs:domain
			rdf:resource="&fibo-fnd-dt-oc;Occurrence"/>
		<rdfs:range
			rdf:resource="&fibo-fnd-dt-oc;Occurrence"/>
		<skos:definition>Related an Occurrence to another Occurrence, most often in the context of communication.</skos:definition>
	</owl:ObjectProperty>
	
	<owl:ObjectProperty
		rdf:about="&fibo-ln-ln-up;fnd-thingRequested">
	</owl:ObjectProperty>
	
	<owl:ObjectProperty
		rdf:about="&fibo-ln-ln-up;hasActualUnpaidBalance">
		<rdfs:subPropertyOf
			rdf:resource="&fibo-fnd-rel-rel;has"/>
		<rdfs:range
			rdf:resource="&fibo-fnd-acc-cur;MonetaryAmount"/>
		<skos:definition>What the actual balance is after a payment is made.</skos:definition>
		<skos:editorialNote>Topic: Payments</skos:editorialNote>
	</owl:ObjectProperty>
	
	<owl:ObjectProperty
		rdf:about="&fibo-ln-ln-up;hasAppraiser">
		<rdfs:subPropertyOf
			rdf:resource="&fibo-ln-ln-up;hasParticipant"/>
		<skos:definition>Relates e.g. an appraisal, to a party that plays the role of conducting a property appraisal.</skos:definition>
	</owl:ObjectProperty>
	
	<owl:ObjectProperty
		rdf:about="&fibo-ln-ln-up;hasCreationDate">
		<rdfs:subPropertyOf
			rdf:resource="&fibo-fnd-dt-fd;hasStartDate"/>
		<skos:definition>LC to check: Relates something to the date when it came into existence.</skos:definition>
	</owl:ObjectProperty>
	
	<owl:ObjectProperty
		rdf:about="&fibo-ln-ln-up;hasDateReceived">
		<rdfs:subPropertyOf
			rdf:resource="&fibo-fnd-dt-fd;hasDate"/>
		<skos:definition>LC to check: Relates something to the date when it was received, e.g. a loan application request.</skos:definition>
	</owl:ObjectProperty>
	
	<owl:ObjectProperty
		rdf:about="&fibo-ln-ln-up;hasIndividualContactInfo">
		<rdfs:range
			rdf:resource="&fibo-ln-ln-up;ContactInfo"/>
		<skos:definition>Relates something to the contact information of an individual (as opposed to an organization).</skos:definition>
		<skos:editorialNote>Topic: BE</skos:editorialNote>
	</owl:ObjectProperty>
	
	<owl:ObjectProperty
		rdf:about="&fibo-ln-ln-up;hasInput">
		<rdfs:subPropertyOf
			rdf:resource="&fibo-ln-ln-up;hasParticipant"/>
		<owl:inverseOf
			rdf:resource="&fibo-ln-ln-up;hasInputOn"/>
		<skos:definition>Relates an Occurrence to something that is used as an input to some activity or process.</skos:definition>
	</owl:ObjectProperty>
	
	<owl:ObjectProperty
		rdf:about="&fibo-ln-ln-up;hasInputOn">
	</owl:ObjectProperty>
	
	<owl:ObjectProperty
		rdf:about="&fibo-ln-ln-up;hasInterestRate">
		<rdfs:subPropertyOf
			rdf:resource="&fibo-fnd-rel-rel;has"/>
		<skos:definition>Relates, e.g. a loan, to an insterest rate.</skos:definition>
		<skos:editorialNote>Topic: Payments</skos:editorialNote>
	</owl:ObjectProperty>
	
	<owl:ObjectProperty
		rdf:about="&fibo-ln-ln-up;hasItemInspected">
		<rdfs:subPropertyOf
			rdf:resource="&fibo-ln-ln-up;hasParticipant"/>
		<skos:definition>Relates an Inspection to the thing being inspected.</skos:definition>
	</owl:ObjectProperty>
	
	<owl:ObjectProperty
		rdf:about="&fibo-ln-ln-up;hasItemOffered">
		<rdfs:subPropertyOf
			rdf:resource="&fibo-ln-ln-up;hasParticipant"/>
		<skos:definition>Relates an Offer to the item on offer</skos:definition>
	</owl:ObjectProperty>
	
	<owl:DatatypeProperty
		rdf:about="&fibo-ln-ln-up;hasNumberOfEntries">
		<rdfs:subPropertyOf
			rdf:resource="&fibo-ln-ln-up;rel-hasCount"/>
		<rdfs:range
			rdf:resource="&xs;positiveInteger"/>
		<skos:definition>The number of entries, e.g. in a report.</skos:definition>
	</owl:DatatypeProperty>
	
	<owl:ObjectProperty
		rdf:about="&fibo-ln-ln-up;hasObligee">
		<rdfs:subPropertyOf
			rdf:resource="&fibo-ln-ln-up;hasPartyWithRight"/>
		<skos:definition>Relates e.g. an agreement or commitment to a party legally entitled to receive a payment.</skos:definition>
	</owl:ObjectProperty>
	
	<owl:ObjectProperty
		rdf:about="&fibo-ln-ln-up;hasObligor">
		<rdfs:subPropertyOf
			rdf:resource="&fibo-ln-ln-up;hasPartyWithDuty"/>
		<skos:definition>Relates e.g. an agreement or commitment to a party who is legally obliged to the other party  (e.g. the one who must may loan payments)</skos:definition>
	</owl:ObjectProperty>
	
	<owl:ObjectProperty
		rdf:about="&fibo-ln-ln-up;hasOrgContactInfo">
		<rdfs:range
			rdf:resource="&fibo-ln-ln-up;ContactInfo"/>
		<skos:definition>Relates something to the contact information of an organization  (as opposed to an individual).</skos:definition>
		<skos:editorialNote>Topic: BE</skos:editorialNote>
	</owl:ObjectProperty>
	
	<owl:ObjectProperty
		rdf:about="&fibo-ln-ln-up;hasOutput">
		<rdfs:subPropertyOf
			rdf:resource="&fibo-ln-ln-up;hasParticipant"/>
		<owl:inverseOf
			rdf:resource="&fibo-ln-ln-up;hasOutputOn"/>
		<skos:definition>Relates an Occurrence to something that is the result of some activity or process.</skos:definition>
	</owl:ObjectProperty>
	
	<owl:ObjectProperty
		rdf:about="&fibo-ln-ln-up;hasOutputOn">
	</owl:ObjectProperty>
	
	<owl:ObjectProperty
		rdf:about="&fibo-ln-ln-up;hasParticipant">
		<skos:definition>Relates e.g. an agreement or event to an object or party playing a role.</skos:definition>
	</owl:ObjectProperty>
	
	<owl:ObjectProperty
		rdf:about="&fibo-ln-ln-up;hasPartyWithDuty">
		<rdfs:subPropertyOf
			rdf:resource="&fibo-ln-ln-up;hasParticipant"/>
		<rdfs:range
			rdf:resource="&fibo-fnd-pty-pty;IndependentParty"/>
		<skos:definition>Relates e.g. an agreement or commitment to a party who is obliged in some way to the other party (e.g. the one who owes funds on a payment obligation)</skos:definition>
	</owl:ObjectProperty>
	
	<owl:ObjectProperty
		rdf:about="&fibo-ln-ln-up;hasPartyWithRight">
		<rdfs:subPropertyOf
			rdf:resource="&fibo-ln-ln-up;hasParticipant"/>
		<rdfs:range
			rdf:resource="&fibo-fnd-pty-pty;IndependentParty"/>
		<skos:definition>Relates e.g. an agreement or commitment to a party with a right regarding what the other party is obliged to do  (e.g. the one with the right to receive funds regarding a payment obligation)</skos:definition>
	</owl:ObjectProperty>
	
	<owl:ObjectProperty
		rdf:about="&fibo-ln-ln-up;hasPayee">
		<rdfs:subPropertyOf
			rdf:resource="&fibo-ln-ln-up;hasPartyWithRight"/>
		<skos:definition>Relates e.g. an agreement or commitment to a party who is (or is intended to be) entitled to receive a payment.</skos:definition>
	</owl:ObjectProperty>
	
	<owl:ObjectProperty
		rdf:about="&fibo-ln-ln-up;hasPayor">
		<rdfs:subPropertyOf
			rdf:resource="&fibo-ln-ln-up;hasPartyWithDuty"/>
		<skos:definition>Relates e.g. an agreement or commitment to a party who is (or is intended to be) obliged to pay the other party  (e.g. the one who must may loan payments)</skos:definition>
	</owl:ObjectProperty>
	
	<owl:ObjectProperty
		rdf:about="&fibo-ln-ln-up;hasScheduledUnpaidBalance">
		<rdfs:subPropertyOf
			rdf:resource="&fibo-fnd-rel-rel;has"/>
		<rdfs:range
			rdf:resource="&fibo-fnd-acc-cur;MonetaryAmount"/>
		<skos:definition>What the unpaid balance should be when a scheduled payment is made according to contract terms</skos:definition>
		<skos:editorialNote>Topic: Payments</skos:editorialNote>
	</owl:ObjectProperty>
	
	<owl:ObjectProperty
		rdf:about="&fibo-ln-ln-up;hasSeniorAppraiser">
		<rdfs:subPropertyOf
			rdf:resource="&fibo-ln-ln-up;hasParticipant"/>
		<skos:definition>Relates e.g. an appraisal to the appraiser with seniority or supervisory responsibilities.</skos:definition>
	</owl:ObjectProperty>
	
	<owl:DatatypeProperty
		rdf:about="&fibo-ln-ln-up;hasString">
		<rdfs:range
			rdf:resource="&xs;string"/>
		<skos:definition>A general purpose property pointing from a text object to its string.</skos:definition>
		<skos:editorialNote>TODO:  change name of fibo-fnd-rel-rel:hasUniqueIdentifier to hasUniqueString to avoid confusion with the class, Identifier.</skos:editorialNote>
		<skos:editorialNote>TODO: make a superproperty of fibo-fnd-rel-rel:hasUniqueIdentifier</skos:editorialNote>
	</owl:DatatypeProperty>
	
	<owl:ObjectProperty
		rdf:about="&fibo-ln-ln-up;instantiates">
		<skos:definition>Iis an instantiation of e.g. a template, offer or form.</skos:definition>
	</owl:ObjectProperty>
	
	<owl:ObjectProperty
		rdf:about="&fibo-ln-ln-up;isEvidencedBy_g">
		<skos:definition>A more generic version of the property in the contracts ontology which has domain:WrittenContract and range ContractDocument.</skos:definition>
	</owl:ObjectProperty>
	
	<owl:ObjectProperty
		rdf:about="&fibo-ln-ln-up;opty-isGuaranteedBy">
	</owl:ObjectProperty>
	
	<owl:Class
		rdf:about="&fibo-ln-ln-up;pas-LineItem">
		<rdfs:subClassOf
			rdf:resource="&fibo-ln-ln-up;Specification"/>
		<rdfs:subClassOf>
			<owl:Restriction>
				<owl:minQualifiedCardinality
					rdf:datatype="&xs;nonNegativeInteger">0</owl:minQualifiedCardinality>
				<owl:onClass
					rdf:resource="&fibo-fnd-acc-cur;MonetaryAmount"/>
				<owl:onProperty
					rdf:resource="&fibo-ln-ln-up;pas-hasUnitCost"/>
			</owl:Restriction>
		</rdfs:subClassOf>
		<rdfs:subClassOf>
			<owl:Restriction>
				<owl:minQualifiedCardinality
					rdf:datatype="&xs;nonNegativeInteger">0</owl:minQualifiedCardinality>
				<owl:onDataRange
					rdf:resource="&xs;positiveInteger"/>
				<owl:onProperty
					rdf:resource="&fibo-fnd-dt-fd;hasCount"/>
			</owl:Restriction>
		</rdfs:subClassOf>
		<rdfs:subClassOf>
			<owl:Restriction>
				<owl:onProperty
					rdf:resource="&fibo-fnd-rel-rel;has"/>
				<owl:someValuesFrom>
					<owl:Class>
						<owl:unionOf>
							<rdf:Description>
								<rdf:first
									rdf:resource="&fibo-fnd-pas-pas;Product"/>
								<rdf:rest>
									<rdf:Description>
										<rdf:first
											rdf:resource="&fibo-ln-ln-up;ChargeCategory"/>
										<rdf:rest
											rdf:resource="&rdf;nil"/>
									</rdf:Description>
								</rdf:rest>
							</rdf:Description>
						</owl:unionOf>
					</owl:Class>
				</owl:someValuesFrom>
			</owl:Restriction>
		</rdfs:subClassOf>
		<rdfs:subClassOf>
			<owl:Restriction>
				<owl:onProperty
					rdf:resource="&fibo-ln-ln-up;pas-hasCost"/>
				<owl:someValuesFrom
					rdf:resource="&fibo-fnd-acc-cur;MonetaryAmount"/>
			</owl:Restriction>
		</rdfs:subClassOf>
		<skos:definition>A description of a product or service including its unit cost, number of units and total cost.</skos:definition>
	</owl:Class>
	
	<owl:Class
		rdf:about="&fibo-ln-ln-up;pas-MarketCategory">
		<rdfs:subClassOf
			rdf:resource="&fibo-fnd-arr-cls;Classifier"/>
		<skos:definition>Specifies the market domain in which a product is offered.</skos:definition>
	</owl:Class>
	
	<owl:ObjectProperty
		rdf:about="&fibo-ln-ln-up;pas-hasChargeCategory">
		<rdfs:subPropertyOf
			rdf:resource="&fibo-fnd-rel-rel;has"/>
	</owl:ObjectProperty>
	
	<owl:ObjectProperty
		rdf:about="&fibo-ln-ln-up;pas-hasCost">
		<rdfs:subPropertyOf
			rdf:resource="&fibo-ln-ln-up;cur-hasAmount"/>
		<skos:definition>Relates an item to its cost, it can entail adding up other costs (e.g. 4 units * a unit price)</skos:definition>
	</owl:ObjectProperty>
	
	<owl:ObjectProperty
		rdf:about="&fibo-ln-ln-up;pas-hasProduct">
		<rdfs:subPropertyOf
			rdf:resource="&fibo-fnd-rel-rel;has"/>
	</owl:ObjectProperty>
	
	<owl:ObjectProperty
		rdf:about="&fibo-ln-ln-up;pas-hasUnitCost">
	</owl:ObjectProperty>
	
	<owl:ObjectProperty
		rdf:about="&fibo-ln-ln-up;pas-hasUnitPrice">
		<rdfs:subPropertyOf
			rdf:resource="&fibo-ln-ln-up;cur-hasAmount"/>
		<skos:definition>Relates an item to its unit cost</skos:definition>
	</owl:ObjectProperty>
	
	<owl:Class
		rdf:about="&fibo-ln-ln-up;pas-mfu-Offer">
		<rdfs:subClassOf
			rdf:resource="&fibo-fnd-agr-agr;Commitment"/>
		<skos:definition>A commitment to provide a product or service for an agreed price, if a buyer comes along.</skos:definition>
		<skos:editorialNote>TODO: model this out properly, add to products and services ontology.</skos:editorialNote>
	</owl:Class>
	
	<owl:ObjectProperty
		rdf:about="&fibo-ln-ln-up;performedBy">
		<rdfs:subPropertyOf
			rdf:resource="&fibo-ln-ln-up;hasParticipant"/>
		<skos:definition>Relates an Occurrence to a party that fully or partially performs the activity or process corresponding to the Occurrence.  Eg. who performed an Inspection.</skos:definition>
	</owl:ObjectProperty>
	
	<owl:Class
		rdf:about="&fibo-ln-ln-up;pty-CreditReportingAgency_I">
		<rdfs:subClassOf
			rdf:resource="&fibo-fnd-pty-pty;IndependentParty"/>
		<skos:definition>This is the independent party, not the party in role</skos:definition>
		<skos:editorialNote>Lynn: todo</skos:editorialNote>
	</owl:Class>
	
	<owl:Class
		rdf:about="&fibo-ln-ln-up;pty-CreditRepository_I">
		<rdfs:subClassOf
			rdf:resource="&fibo-fnd-pty-pty;IndependentParty"/>
		<skos:definition>This is the independent party, not the party in role</skos:definition>
		<skos:editorialNote>Lynn: todo</skos:editorialNote>
	</owl:Class>
	
	<owl:ObjectProperty
		rdf:about="&fibo-ln-ln-up;pty-IndependentParty">
		<rdfs:label>pty-independent party</rdfs:label>
	</owl:ObjectProperty>
	
	<owl:ObjectProperty
		rdf:about="&fibo-ln-ln-up;rel-from">
	</owl:ObjectProperty>
	
	<owl:DatatypeProperty
		rdf:about="&fibo-ln-ln-up;rel-hasCount">
		<rdfs:range
			rdf:resource="&xs;positiveInteger"/>
		<skos:definition>The count of the number of something, e.g. entries in a schedule.</skos:definition>
		<skos:editorialNote>fibo-fnd-dt-fd:hasCount should probably be replaced with this more generic version, or if not made a subproperty of it.</skos:editorialNote>
	</owl:DatatypeProperty>
	
	<owl:DatatypeProperty
		rdf:about="&fibo-ln-ln-up;rel-hasVersion">
		<rdfs:range
			rdf:resource="&xs;string"/>
		<skos:definition>Indicates the version for something.</skos:definition>
	</owl:DatatypeProperty>
	
	<owl:ObjectProperty
		rdf:about="&fibo-ln-ln-up;rel-isInformedBy">
		<skos:definition>Relates, e.g. a  valuation to something that is  used to inform the valuation.</skos:definition>
	</owl:ObjectProperty>
	
	<owl:ObjectProperty
		rdf:about="&fibo-ln-ln-up;rel-isOf">
		<owl:inverseOf
			rdf:resource="&fibo-fnd-rel-rel;has"/>
		<skos:definition>Inverse of fibo-fnd-rel-rel:has</skos:definition>
		<skos:editorialNote></skos:editorialNote>
	</owl:ObjectProperty>
	
	<owl:ObjectProperty
		rdf:about="&fibo-ln-ln-up;rel-isProducedBy_I">
		<owl:inverseOf
			rdf:resource="&fibo-ln-ln-up;rel-produces_I"/>
		<skos:definition>Indicates who or what produced something.</skos:definition>
		<skos:editorialNote>Ideally, this would be a superproperty of pas:isProducedBy in products and services ontology, but that is reserved for use with ThingInRole.  This property is therefore a superproperty of an unnamed property chain from the thing produced  to the independent producing thing that goes through an instance of a class that means PartyInProducerRole.</skos:editorialNote>
	</owl:ObjectProperty>
	
	<owl:ObjectProperty
		rdf:about="&fibo-ln-ln-up;rel-isSubmittedBy">
		<rdfs:range
			rdf:resource="&fibo-fnd-aap-agt;AutonomousAgent"/>
		<skos:definition>Relates a Report to the Agent that is providing the Report</skos:definition>
		<skos:editorialNote>Ideally, this would be a subproperty of isProvidedBy, but that is reserved for use with ThingInRole.  This property is therefore a subproperty of an unnamed property chain from the thing submitted to the submitting  institution that goes through an instance of a class that means PartyInProviderRole.</skos:editorialNote>
	</owl:ObjectProperty>
	
	<owl:ObjectProperty
		rdf:about="&fibo-ln-ln-up;rel-isSubmittedTo">
		<rdfs:range
			rdf:resource="&fibo-fnd-aap-agt;AutonomousAgent"/>
		<skos:definition>Relates a Report to the Agent that is receiving the Report</skos:definition>
	</owl:ObjectProperty>
	
	<owl:ObjectProperty
		rdf:about="&fibo-ln-ln-up;rel-produces_I">
	</owl:ObjectProperty>
	
	<owl:ObjectProperty
		rdf:about="&fibo-ln-ln-up;rel-to">
	</owl:ObjectProperty>
	
	<owl:ObjectProperty
		rdf:about="&fibo-ln-ln-up;rel-uses_g">
		<skos:definition>Indicates who or what produced something.</skos:definition>
		<skos:editorialNote>Check to see if this is still used.</skos:editorialNote>
		<skos:editorialNote>This is a generic version of the fibo-fnd-rel-rel:uses property whose domain is too narrow.  If they fix it, this should be chagned to fibo-fnd-rel-rel:uses.</skos:editorialNote>
	</owl:ObjectProperty>
	
	<owl:ObjectProperty
		rdf:about="&fibo-ln-ln-up;thingBeingValued">
	</owl:ObjectProperty>
	
	<owl:ObjectProperty
		rdf:about="&fibo-ln-ln-up;worksFor">
		<rdfs:domain
			rdf:resource="&fibo-fnd-aap-ppl;LegallyCapablePerson"/>
		<rdfs:range
			rdf:resource="&fibo-fnd-pty-pty;IndependentParty"/>
		<skos:definition>Indicates that a person works for some other person or company. Different arrangements are possible, e.g. employee or contractor.</skos:definition>
	</owl:ObjectProperty>

</rdf:RDF>