<?xml version="1.0" encoding="UTF-8"?>
<!DOCTYPE rdf:RDF [
	<!ENTITY dct "http://purl.org/dc/terms/">
	<!ENTITY fibo-civ-fnd-civ "https://spec.edmcouncil.org/fibo/ontology/CIV/Funds/CIV/">
	<!ENTITY fibo-fnd-rel-rel "https://spec.edmcouncil.org/fibo/ontology/FND/Relations/Relations/">
	<!ENTITY fibo-fnd-utl-av "https://spec.edmcouncil.org/fibo/ontology/FND/Utilities/AnnotationVocabulary/">
	<!ENTITY fibo-sec-dbt-ab-spv "https://spec.edmcouncil.org/fibo/ontology/SEC/Debt/AssetBackedSecurities/AssetBackedSPVs/">
	<!ENTITY owl "http://www.w3.org/2002/07/owl#">
	<!ENTITY rdf "http://www.w3.org/1999/02/22-rdf-syntax-ns#">
	<!ENTITY rdfs "http://www.w3.org/2000/01/rdf-schema#">
	<!ENTITY skos "http://www.w3.org/2004/02/skos/core#">
	<!ENTITY xsd "http://www.w3.org/2001/XMLSchema#">
]>
<rdf:RDF xml:base="https://spec.edmcouncil.org/fibo/ontology/SEC/Debt/AssetBackedSecurities/AssetBackedSPVs/"
	xmlns:dct="http://purl.org/dc/terms/"
	xmlns:fibo-civ-fnd-civ="https://spec.edmcouncil.org/fibo/ontology/CIV/Funds/CIV/"
	xmlns:fibo-fnd-rel-rel="https://spec.edmcouncil.org/fibo/ontology/FND/Relations/Relations/"
	xmlns:fibo-fnd-utl-av="https://spec.edmcouncil.org/fibo/ontology/FND/Utilities/AnnotationVocabulary/"
	xmlns:fibo-sec-dbt-ab-spv="https://spec.edmcouncil.org/fibo/ontology/SEC/Debt/AssetBackedSecurities/AssetBackedSPVs/"
	xmlns:owl="http://www.w3.org/2002/07/owl#"
	xmlns:rdf="http://www.w3.org/1999/02/22-rdf-syntax-ns#"
	xmlns:rdfs="http://www.w3.org/2000/01/rdf-schema#"
	xmlns:skos="http://www.w3.org/2004/02/skos/core#"
	xmlns:xsd="http://www.w3.org/2001/XMLSchema#">
	
	<owl:Ontology rdf:about="https://spec.edmcouncil.org/fibo/ontology/SEC/Debt/AssetBackedSecurities/AssetBackedSPVs/">
		<rdfs:label xml:lang="en">AssetBackedSPVs</rdfs:label>
		<dct:abstract>Special purpose vehicles used in the issuance of asset backed securities.</dct:abstract>
		<owl:imports rdf:resource="https://spec.edmcouncil.org/fibo/ontology/CIV/Funds/CIV/"/>
		<owl:imports rdf:resource="https://spec.edmcouncil.org/fibo/ontology/FND/Utilities/AnnotationVocabulary/"/>
		<owl:imports rdf:resource="https://spec.edmcouncil.org/fibo/ontology/SEC/Securities/Pools/"/>
		<owl:versionIRI rdf:resource="https://spec.edmcouncil.org/fibo/ontology/SEC/Debt/AssetBackedSecurities/AssetBackedSPVs/"/>
		<fibo-fnd-utl-av:hasMaturityLevel rdf:resource="&fibo-fnd-utl-av;Provisional"/>
	</owl:Ontology>
	
	<owl:Class rdf:about="&fibo-sec-dbt-ab-spv;DebtSPV">
		<rdfs:subClassOf rdf:resource="&fibo-civ-fnd-civ;SpecialPurposeVehicle"/>
		<rdfs:subClassOf>
			<owl:Restriction>
				<owl:onProperty rdf:resource="&fibo-civ-fnd-civ;isSetUpFor"/>
				<owl:someValuesFrom rdf:resource="&fibo-sec-dbt-ab-spv;DebtSecuritiesIssuance"/>
			</owl:Restriction>
		</rdfs:subClassOf>
		<rdfs:subClassOf>
			<owl:Restriction>
				<owl:onProperty rdf:resource="&fibo-fnd-rel-rel;comprises"/>
				<owl:someValuesFrom rdf:resource="https://spec.edmcouncil.org/fibo/ontology/SEC/Debt/AssetBackedSecurities/PoolBackedSecurities/SecuritizedDebtPool"/>
			</owl:Restriction>
		</rdfs:subClassOf>
		<rdfs:label xml:lang="en">debt s p v</rdfs:label>
		<skos:definition xml:lang="en">A Special Purpose Vehicle (SPV) set up specifically to issue a debt security or securities. It is set up by a company or a group of companies to create instruments that are off the company&apos;s balance sheet.</skos:definition>
		<fibo-fnd-utl-av:explanatoryNote xml:lang="en">The SPV exists for a specific period of time and is then disbanded. It may take the form of an LLC or other legal entity. Special Purpose Vehicles are also referred to as bankruptcy remote entities, as they isolate financial risk.</fibo-fnd-utl-av:explanatoryNote>
	</owl:Class>
	
	<owl:Class rdf:about="&fibo-sec-dbt-ab-spv;DebtSecuritiesIssuance">
		<rdfs:subClassOf rdf:resource="&fibo-sec-dbt-ab-spv;SecuritiesIssuance"/>
		<rdfs:label xml:lang="en">debt securities issuance</rdfs:label>
		<skos:definition xml:lang="en">SPV set up to issue debt instruments such as for structured finance.</skos:definition>
	</owl:Class>
	
	<owl:Class rdf:about="&fibo-sec-dbt-ab-spv;SecuritiesIssuance">
		<rdfs:subClassOf rdf:resource="&fibo-civ-fnd-civ;SPVPurpose"/>
		<rdfs:label xml:lang="en">securities issuance</rdfs:label>
		<skos:definition xml:lang="en">The SPV is set up to issue securities.</skos:definition>
	</owl:Class>
	
	<owl:Class rdf:about="&fibo-sec-dbt-ab-spv;SecuritiesIssuanceSPV">
		<rdfs:subClassOf rdf:resource="&fibo-civ-fnd-civ;SpecialPurposeVehicle"/>
		<rdfs:subClassOf>
			<owl:Restriction>
				<owl:onProperty rdf:resource="&fibo-civ-fnd-civ;isSetUpFor"/>
				<owl:someValuesFrom rdf:resource="&fibo-sec-dbt-ab-spv;SecuritiesIssuance"/>
			</owl:Restriction>
		</rdfs:subClassOf>
		<rdfs:subClassOf>
			<owl:Restriction>
				<owl:onProperty rdf:resource="&fibo-fnd-rel-rel;comprises"/>
				<owl:someValuesFrom rdf:resource="https://spec.edmcouncil.org/fibo/ontology/SEC/Debt/AssetBackedSecurities/PoolBackedSecurities/SecuritizedDebtPool"/>
			</owl:Restriction>
		</rdfs:subClassOf>
		<rdfs:label xml:lang="en">securities issuance s p v</rdfs:label>
		<skos:definition xml:lang="en">An SPV set up specifically to issue securities.</skos:definition>
	</owl:Class>
	
	<owl:DatatypeProperty rdf:about="&fibo-sec-dbt-ab-spv;isREMIC">
		<rdfs:label xml:lang="en">is r e m i c</rdfs:label>
		<rdfs:domain rdf:resource="&fibo-sec-dbt-ab-spv;DebtSPV"/>
		<rdfs:range rdf:resource="&xsd;boolean"/>
		<skos:definition xml:lang="en">Whether the SPV is set up and registered as a Real Estate Mortgage Investment Conduit (REMIC). REMICs are a type of special purpose vehicle used for the pooling of mortgage loans and issuance of mortgage-backed securities. They are defined under the United States Internal Revenue Code (Tax Reform Act of 1986), and are the typical vehicle of choice for the securitization of residential mortgages in the US.</skos:definition>
	</owl:DatatypeProperty>

</rdf:RDF>