<?xml version="1.0" encoding="UTF-8"?>
<!DOCTYPE rdf:RDF [
	<!ENTITY dct "http://purl.org/dc/terms/">
	<!ENTITY fibo-fbc-dae-dbt "https://spec.edmcouncil.org/fibo/ontology/FBC/DebtAndEquities/Debt/">
	<!ENTITY fibo-fnd-acc-cur "https://spec.edmcouncil.org/fibo/ontology/FND/Accounting/CurrencyAmount/">
	<!ENTITY fibo-fnd-arr-arr "https://spec.edmcouncil.org/fibo/ontology/FND/Arrangements/Arrangements/">
	<!ENTITY fibo-fnd-oac-own "https://spec.edmcouncil.org/fibo/ontology/FND/OwnershipAndControl/Ownership/">
	<!ENTITY fibo-fnd-utl-alx "https://spec.edmcouncil.org/fibo/ontology/FND/Utilities/Analytics/">
	<!ENTITY fibo-fnd-utl-av "https://spec.edmcouncil.org/fibo/ontology/FND/Utilities/AnnotationVocabulary/">
	<!ENTITY fibo-ind-ei-ei "https://spec.edmcouncil.org/fibo/ontology/IND/EconomicIndicators/EconomicIndicators/">
	<!ENTITY fibo-ind-ind-ind "https://spec.edmcouncil.org/fibo/ontology/IND/Indicators/Indicators/">
	<!ENTITY fibo-ind-ir-ir "https://spec.edmcouncil.org/fibo/ontology/IND/InterestRates/InterestRates/">
	<!ENTITY fibo-loan-typ-prod "https://spec.edmcouncil.org/fibo/ontology/LOAN/LoanTypes/LoanProducts/">
	<!ENTITY fibo-sec-dbt-ab-abs "https://spec.edmcouncil.org/fibo/ontology/SEC/Debt/AssetBackedSecurities/AssetBackedSecurities/">
	<!ENTITY fibo-sec-dbt-ab-cdo "https://spec.edmcouncil.org/fibo/ontology/SEC/Debt/AssetBackedSecurities/CDOs/">
	<!ENTITY fibo-sec-dbt-ab-mbs "https://spec.edmcouncil.org/fibo/ontology/SEC/Debt/AssetBackedSecurities/MortgageBackedSecurities/">
	<!ENTITY fibo-sec-dbt-ab-pbs "https://spec.edmcouncil.org/fibo/ontology/SEC/Debt/AssetBackedSecurities/PoolBackedSecurities/">
	<!ENTITY fibo-sec-dbt-ab-spv "https://spec.edmcouncil.org/fibo/ontology/SEC/Debt/AssetBackedSecurities/AssetBackedSPVs/">
	<!ENTITY fibo-sec-dbt-bnd "https://spec.edmcouncil.org/fibo/ontology/SEC/Debt/Bonds/">
	<!ENTITY fibo-sec-dbt-dbti "https://spec.edmcouncil.org/fibo/ontology/SEC/Debt/DebtInstruments/">
	<!ENTITY owl "http://www.w3.org/2002/07/owl#">
	<!ENTITY rdf "http://www.w3.org/1999/02/22-rdf-syntax-ns#">
	<!ENTITY rdfs "http://www.w3.org/2000/01/rdf-schema#">
	<!ENTITY skos "http://www.w3.org/2004/02/skos/core#">
	<!ENTITY xsd "http://www.w3.org/2001/XMLSchema#">
]>
<rdf:RDF xml:base="https://spec.edmcouncil.org/fibo/ontology/SEC/Debt/AssetBackedSecurities/AssetBackedSecurities/"
	xmlns:dct="http://purl.org/dc/terms/"
	xmlns:fibo-fbc-dae-dbt="https://spec.edmcouncil.org/fibo/ontology/FBC/DebtAndEquities/Debt/"
	xmlns:fibo-fnd-acc-cur="https://spec.edmcouncil.org/fibo/ontology/FND/Accounting/CurrencyAmount/"
	xmlns:fibo-fnd-arr-arr="https://spec.edmcouncil.org/fibo/ontology/FND/Arrangements/Arrangements/"
	xmlns:fibo-fnd-oac-own="https://spec.edmcouncil.org/fibo/ontology/FND/OwnershipAndControl/Ownership/"
	xmlns:fibo-fnd-utl-alx="https://spec.edmcouncil.org/fibo/ontology/FND/Utilities/Analytics/"
	xmlns:fibo-fnd-utl-av="https://spec.edmcouncil.org/fibo/ontology/FND/Utilities/AnnotationVocabulary/"
	xmlns:fibo-ind-ei-ei="https://spec.edmcouncil.org/fibo/ontology/IND/EconomicIndicators/EconomicIndicators/"
	xmlns:fibo-ind-ind-ind="https://spec.edmcouncil.org/fibo/ontology/IND/Indicators/Indicators/"
	xmlns:fibo-ind-ir-ir="https://spec.edmcouncil.org/fibo/ontology/IND/InterestRates/InterestRates/"
	xmlns:fibo-loan-typ-prod="https://spec.edmcouncil.org/fibo/ontology/LOAN/LoanTypes/LoanProducts/"
	xmlns:fibo-sec-dbt-ab-abs="https://spec.edmcouncil.org/fibo/ontology/SEC/Debt/AssetBackedSecurities/AssetBackedSecurities/"
	xmlns:fibo-sec-dbt-ab-cdo="https://spec.edmcouncil.org/fibo/ontology/SEC/Debt/AssetBackedSecurities/CDOs/"
	xmlns:fibo-sec-dbt-ab-mbs="https://spec.edmcouncil.org/fibo/ontology/SEC/Debt/AssetBackedSecurities/MortgageBackedSecurities/"
	xmlns:fibo-sec-dbt-ab-pbs="https://spec.edmcouncil.org/fibo/ontology/SEC/Debt/AssetBackedSecurities/PoolBackedSecurities/"
	xmlns:fibo-sec-dbt-ab-spv="https://spec.edmcouncil.org/fibo/ontology/SEC/Debt/AssetBackedSecurities/AssetBackedSPVs/"
	xmlns:fibo-sec-dbt-bnd="https://spec.edmcouncil.org/fibo/ontology/SEC/Debt/Bonds/"
	xmlns:fibo-sec-dbt-dbti="https://spec.edmcouncil.org/fibo/ontology/SEC/Debt/DebtInstruments/"
	xmlns:owl="http://www.w3.org/2002/07/owl#"
	xmlns:rdf="http://www.w3.org/1999/02/22-rdf-syntax-ns#"
	xmlns:rdfs="http://www.w3.org/2000/01/rdf-schema#"
	xmlns:skos="http://www.w3.org/2004/02/skos/core#"
	xmlns:xsd="http://www.w3.org/2001/XMLSchema#">
	
	<owl:Ontology rdf:about="https://spec.edmcouncil.org/fibo/ontology/SEC/Debt/AssetBackedSecurities/AssetBackedSecurities/">
		<rdfs:label xml:lang="en">AssetBackedSecurities</rdfs:label>
		<dct:abstract>Debt securities backed by a pool of assets, including loans of various kinds, credit card pools and home equity lines of credit, as well as esoteric assets.</dct:abstract>
		<owl:imports rdf:resource="https://spec.edmcouncil.org/fibo/ontology/BE/FunctionalEntities/FunctionalEntities/"/>
		<owl:imports rdf:resource="https://spec.edmcouncil.org/fibo/ontology/FBC/DebtAndEquities/Debt/"/>
		<owl:imports rdf:resource="https://spec.edmcouncil.org/fibo/ontology/FND/Accounting/CurrencyAmount/"/>
		<owl:imports rdf:resource="https://spec.edmcouncil.org/fibo/ontology/FND/Arrangements/Arrangements/"/>
		<owl:imports rdf:resource="https://spec.edmcouncil.org/fibo/ontology/FND/OwnershipAndControl/Ownership/"/>
		<owl:imports rdf:resource="https://spec.edmcouncil.org/fibo/ontology/FND/Utilities/Analytics/"/>
		<owl:imports rdf:resource="https://spec.edmcouncil.org/fibo/ontology/FND/Utilities/AnnotationVocabulary/"/>
		<owl:imports rdf:resource="https://spec.edmcouncil.org/fibo/ontology/IND/EconomicIndicators/EconomicIndicators/"/>
		<owl:imports rdf:resource="https://spec.edmcouncil.org/fibo/ontology/IND/Indicators/Indicators/"/>
		<owl:imports rdf:resource="https://spec.edmcouncil.org/fibo/ontology/IND/InterestRates/InterestRates/"/>
		<owl:imports rdf:resource="https://spec.edmcouncil.org/fibo/ontology/LOAN/LoanTypes/LoanProducts/"/>
		<owl:imports rdf:resource="https://spec.edmcouncil.org/fibo/ontology/SEC/Debt/AssetBackedSecurities/AssetBackedSPVs/"/>
		<owl:imports rdf:resource="https://spec.edmcouncil.org/fibo/ontology/SEC/Debt/AssetBackedSecurities/CDOs/"/>
		<owl:imports rdf:resource="https://spec.edmcouncil.org/fibo/ontology/SEC/Debt/AssetBackedSecurities/MortgageBackedSecurities/"/>
		<owl:imports rdf:resource="https://spec.edmcouncil.org/fibo/ontology/SEC/Debt/AssetBackedSecurities/PoolBackedSecurities/"/>
		<owl:imports rdf:resource="https://spec.edmcouncil.org/fibo/ontology/SEC/Debt/Bonds/"/>
		<owl:imports rdf:resource="https://spec.edmcouncil.org/fibo/ontology/SEC/Debt/DebtInstruments/"/>
		<owl:versionIRI rdf:resource="https://spec.edmcouncil.org/fibo/ontology/SEC/Debt/AssetBackedSecurities/AssetBackedSecurities/"/>
		<fibo-fnd-utl-av:hasMaturityLevel rdf:resource="&fibo-fnd-utl-av;Provisional"/>
	</owl:Ontology>
	
	<owl:Class rdf:about="&fibo-sec-dbt-ab-abs;ABSDeal">
		<rdfs:subClassOf rdf:resource="&fibo-sec-dbt-ab-pbs;PoolBackedSecuritiesDeal"/>
		<rdfs:label xml:lang="en">a b s deal</rdfs:label>
		<skos:definition xml:lang="en">The issue of a series of Cash Asset Backed Security certificates.</skos:definition>
	</owl:Class>
	
	<owl:Class rdf:about="&fibo-sec-dbt-ab-abs;ABSDealProspectus">
		<rdfs:subClassOf rdf:resource="&fibo-sec-dbt-ab-pbs;PoolBackedDealProspectus"/>
		<rdfs:label xml:lang="en">a b s deal prospectus</rdfs:label>
		<skos:definition xml:lang="en">Prospectus describing the terms of the issue and each of the instruments included in the asset backed security issue.</skos:definition>
	</owl:Class>
	
	<owl:Class rdf:about="&fibo-sec-dbt-ab-abs;ABSIssuer">
		<rdfs:subClassOf rdf:resource="&fibo-sec-dbt-ab-pbs;PoolBackedSecurityIssuer"/>
		<rdfs:subClassOf>
			<owl:Restriction>
				<owl:onProperty rdf:resource="&fibo-sec-dbt-ab-abs;describedAs"/>
				<owl:someValuesFrom rdf:resource="&fibo-sec-dbt-ab-spv;DebtSPV"/>
			</owl:Restriction>
		</rdfs:subClassOf>
		<rdfs:label xml:lang="en">a b s issuer</rdfs:label>
		<skos:definition xml:lang="en">The issuer of the (Cash) Asset Backed Security. This is generally a Special Purpose Vehicle set up by a corporation. Further details from riskglossary.com: To create an ABS, a corporation creates a special purpose vehicle to which it sells the assets. While is is common to speak of the corporation as the issuer of the ABS, legally, it is the trust or special purpose vehicle that is the issuer. It sells securities to investors. To protect investors from possible bankruptcy of the corporation, there are three legal safeguards: - Transfer of assets from the corporation is a non-recourse, true sale. - Investors receive a perfected interest in the assets&apos; cash flows. - A non-consolidation legal opinion is obtained certifying that assets of the trust or special purpose vehicle cannot be consolidated with the corporation&apos;s assets in the event of bankruptcy. These same safeguards allow the corporation to remove the assets from its balance sheet. The corporation generally continues to service the assets - collecting interest and principal payments, pursuing delinquencies, etc. It is paid out of asset cash flows for providing these ongoing services.</skos:definition>
	</owl:Class>
	
	<owl:Class rdf:about="&fibo-sec-dbt-ab-abs;AutoLoanABS">
		<rdfs:subClassOf rdf:resource="&fibo-sec-dbt-ab-abs;CashAssetBackedSecurityInstrument"/>
		<rdfs:subClassOf>
			<owl:Restriction>
				<owl:onProperty rdf:resource="&fibo-sec-dbt-ab-abs;hasUnderlyingAssets"/>
				<owl:someValuesFrom rdf:resource="&fibo-sec-dbt-ab-abs;AutoLoanPool"/>
			</owl:Restriction>
		</rdfs:subClassOf>
		<rdfs:label xml:lang="en">auto loan a b s</rdfs:label>
		<skos:definition xml:lang="en">ABS issued by auto finance companies and are backed by underlying pools of auto-related loans or leases.</skos:definition>
		<skos:editorialNote xml:lang="en">Leases not shown at present. Added during later review.</skos:editorialNote>
	</owl:Class>
	
	<owl:Class rdf:about="&fibo-sec-dbt-ab-abs;AutoLoanPool">
		<rdfs:subClassOf rdf:resource="&fibo-sec-dbt-ab-abs;LoanPool"/>
		<rdfs:subClassOf>
			<owl:Restriction>
				<owl:onProperty rdf:resource="&fibo-fnd-arr-arr;hasConstituent"/>
				<owl:someValuesFrom rdf:resource="&fibo-sec-dbt-ab-abs;AutoLoanPoolConstituent"/>
			</owl:Restriction>
		</rdfs:subClassOf>
		<rdfs:subClassOf>
			<owl:Restriction>
				<owl:onProperty rdf:resource="&fibo-sec-dbt-ab-abs;poolHasLoanType"/>
				<owl:someValuesFrom rdf:resource="&fibo-loan-typ-prod;AutoLoanPurpose"/>
			</owl:Restriction>
		</rdfs:subClassOf>
		<rdfs:label xml:lang="en">auto loan pool</rdfs:label>
		<skos:definition xml:lang="en">A loan pool covering automobile-related loans.</skos:definition>
	</owl:Class>
	
	<owl:Class rdf:about="&fibo-sec-dbt-ab-abs;AutoLoanPoolConstituent">
		<rdfs:subClassOf rdf:resource="&fibo-sec-dbt-ab-abs;LoanPoolConstituent"/>
		<rdfs:label xml:lang="en">auto loan pool constituent</rdfs:label>
		<skos:definition xml:lang="en">An auto loan defined as a constituent of an Auto Loan Pool.</skos:definition>
	</owl:Class>
	
	<owl:Class rdf:about="&fibo-sec-dbt-ab-abs;CashAssetBackedSecurityInstrument">
		<rdfs:subClassOf rdf:resource="&fibo-sec-dbt-ab-pbs;PoolBackedSecurityInstrument"/>
		<rdfs:subClassOf>
			<owl:Restriction>
				<owl:onProperty rdf:resource="&fibo-sec-dbt-ab-abs;subordinatedTo"/>
				<owl:onClass rdf:resource="&fibo-sec-dbt-ab-abs;CashAssetBackedSecurityInstrument"/>
				<owl:maxQualifiedCardinality rdf:datatype="&xsd;nonNegativeInteger">1</owl:maxQualifiedCardinality>
			</owl:Restriction>
		</rdfs:subClassOf>
		<rdfs:subClassOf>
			<owl:Restriction>
				<owl:onProperty rdf:resource="&fibo-sec-dbt-ab-abs;hasUnderlyingAssets"/>
				<owl:someValuesFrom>
					<owl:Class>
						<owl:unionOf rdf:parseType="Collection">
							<rdf:Description rdf:about="&fibo-sec-dbt-ab-abs;CreditCardPool">
							</rdf:Description>
							<rdf:Description rdf:about="&fibo-sec-dbt-ab-abs;HomeEquityLineOfCreditPool">
							</rdf:Description>
							<rdf:Description rdf:about="&fibo-sec-dbt-ab-abs;LoanPool">
							</rdf:Description>
						</owl:unionOf>
					</owl:Class>
				</owl:someValuesFrom>
			</owl:Restriction>
		</rdfs:subClassOf>
		<rdfs:subClassOf>
			<owl:Restriction>
				<owl:onProperty rdf:resource="&fibo-sec-dbt-ab-pbs;hasTrancheType"/>
				<owl:someValuesFrom rdf:resource="&fibo-sec-dbt-ab-mbs;TrancheType"/>
			</owl:Restriction>
		</rdfs:subClassOf>
		<rdfs:subClassOf>
			<owl:Restriction>
				<owl:onProperty rdf:resource="&fibo-sec-dbt-ab-pbs;issuedBy"/>
				<owl:someValuesFrom rdf:resource="&fibo-sec-dbt-ab-abs;ABSIssuer"/>
			</owl:Restriction>
		</rdfs:subClassOf>
		<rdfs:label xml:lang="en">cash asset backed security instrument</rdfs:label>
		<owl:disjointWith rdf:resource="&fibo-sec-dbt-ab-cdo;CashCDOTranche"/>
		<owl:disjointWith rdf:resource="&fibo-sec-dbt-ab-mbs;MortgageBackedSecurityInstrument"/>
		<skos:definition xml:lang="en">An asset-backed security is a type of bond or note that is based on pools of assets, or collateralized by the cash flows from a specified pool of underlying assets. Assets are pooled to make otherwise minor and uneconomical investments worthwhile, while also reducing risk by diversifying the underlying assets.</skos:definition>
		<skos:editorialNote xml:lang="en">Definition of ABS is one with any kind of asset underlying which is not a mortgage, e.g. a loan, credit card etc. Asset Backed Securities, for example home equity loans (HEL), credit cards, etc. These are securities backed by receivables [payments] that are either secured (HEL) or unsecured (credit card), tranched on the basis of prepayment and default risks. Action: Determine where mobile home and second mortgage based securities fit in, and add to the relevant definition. Outcome: these would be specialised kinds of pools of loans and are therefore reflected by specific typs of Cash ABS, in the same way as Auto Loan ABS are defined. Note also that an issue of ABS certificates (contracts) may have different tranches which relate to these different kinds of loan, and other as yet undefined types of loan. These are capable of extension into indefinite numbers of loan types / pool types, so it would not be practical to include all the possibilities in the standard terms other than as selectable types of loan in the loan type selection data range.</skos:editorialNote>
	</owl:Class>
	
	<owl:Class rdf:about="&fibo-sec-dbt-ab-abs;ControlledAmortizationBond">
		<rdfs:subClassOf rdf:resource="&fibo-sec-dbt-bnd;AmortizingBond"/>
		<rdfs:subClassOf>
			<owl:Restriction>
				<owl:onProperty rdf:resource="&fibo-sec-dbt-dbti;hasRepaymentTerms"/>
				<owl:someValuesFrom rdf:resource="&fibo-sec-dbt-ab-abs;ControlledAmortizationStructure"/>
			</owl:Restriction>
		</rdfs:subClassOf>
		<rdfs:label>controlled amortization bond</rdfs:label>
		<skos:definition>bond that is securitized using a controlled amortization structure</skos:definition>
		<fibo-fnd-utl-av:adaptedFrom>http://www.investinginbonds.com/learnmore.asp?catid=11&amp;subcatid=57&amp;id=15</fibo-fnd-utl-av:adaptedFrom>
		<fibo-fnd-utl-av:explanatoryNote>Revolving debt (primarily credit card receivables, but also HELOCs, trade receivables, dealer floor-plan loans and some leases) may be securitized using a controlled amortization structure. This is a method of providing investors with a relatively predictable repayment schedule, even though the underlying assets are nonamortizing. Controlled-amortization ABS resemble corporate bonds with a sinking fund. After a predetermined &apos;revolving&apos; period during which only interest payments are made, these securities attempt to return principal to investors in a series of defined periodic payments that usually occur over less than a year. A risk inherent in this kind of ABS is an early amortization event. (See &apos;Early-Amortization Risk&apos;, on page 20.)</fibo-fnd-utl-av:explanatoryNote>
	</owl:Class>
	
	<owl:Class rdf:about="&fibo-sec-dbt-ab-abs;ControlledAmortizationStructure">
		<rdfs:subClassOf rdf:resource="&fibo-sec-dbt-bnd;BondAmortizationPaymentTerms"/>
		<rdfs:label>controlled amortization structure</rdfs:label>
		<skos:definition>method of providing investors with a relatively predictable repayment schedule, even though the underlying assets are nonamortizing</skos:definition>
	</owl:Class>
	
	<owl:Class rdf:about="&fibo-sec-dbt-ab-abs;CreditCardABS">
		<rdfs:subClassOf rdf:resource="&fibo-sec-dbt-ab-abs;CashAssetBackedSecurityInstrument"/>
		<rdfs:subClassOf>
			<owl:Restriction>
				<owl:onProperty rdf:resource="&fibo-sec-dbt-ab-abs;hasUnderlyingAssets"/>
				<owl:someValuesFrom rdf:resource="&fibo-sec-dbt-ab-abs;CreditCardPool"/>
			</owl:Restriction>
		</rdfs:subClassOf>
		<rdfs:label xml:lang="en">credit card a b s</rdfs:label>
		<skos:definition xml:lang="en">These are generally issued by a bank and backed by largely unsecured obligations owed by individuals to the issuer of the card. Definition origin:CESR</skos:definition>
	</owl:Class>
	
	<owl:Class rdf:about="&fibo-sec-dbt-ab-abs;CreditCardPool">
		<rdfs:subClassOf rdf:resource="&fibo-sec-dbt-ab-pbs;PoolOfIndividualDebts"/>
		<rdfs:label xml:lang="en">credit card pool</rdfs:label>
		<owl:disjointWith rdf:resource="&fibo-sec-dbt-ab-abs;LoanPool"/>
	</owl:Class>
	
	<owl:Class rdf:about="&fibo-sec-dbt-ab-abs;EsotericABS">
		<rdfs:subClassOf rdf:resource="&fibo-sec-dbt-ab-abs;CashAssetBackedSecurityInstrument"/>
		<rdfs:subClassOf>
			<owl:Restriction>
				<owl:onProperty rdf:resource="&fibo-sec-dbt-ab-abs;hasUnderlyingCashflow"/>
				<owl:someValuesFrom rdf:resource="&fibo-sec-dbt-ab-abs;PromisedCashFlowAsset"/>
			</owl:Restriction>
		</rdfs:subClassOf>
		<rdfs:label xml:lang="en">esoteric a b s</rdfs:label>
		<skos:definition xml:lang="en">An asset backed security based on some underlying promised future cashflow.</skos:definition>
		<fibo-fnd-utl-av:explanatoryNote xml:lang="en">New example from Goldman Sachs hearing April 2010: Exotic ABS bsaed on box office takings for movies.</fibo-fnd-utl-av:explanatoryNote>
	</owl:Class>
	
	<owl:Class rdf:about="&fibo-sec-dbt-ab-abs;FullyAmortizingBond">
		<rdfs:subClassOf rdf:resource="&fibo-sec-dbt-bnd;AmortizingBond"/>
		<rdfs:label>fully amortizing bond</rdfs:label>
		<skos:definition>amortizing bond that returns principal to investors over the life of the security</skos:definition>
		<fibo-fnd-utl-av:definitionOrigin>http://www.investinginbonds.com/learnmore.asp?catid=11&amp;subcatid=57&amp;id=15</fibo-fnd-utl-av:definitionOrigin>
		<fibo-fnd-utl-av:explanatoryNote>Fully amortizing bonds are designed to closely reflect the full repayment of the underlying loans through scheduled interest and principal payments.</fibo-fnd-utl-av:explanatoryNote>
		<fibo-fnd-utl-av:explanatoryNote>These are typically backed by HELs, auto loans, manufactured-housing contracts and other fully amortizing assets. Prepayment risk is a key consideration with such ABS, although the rate of prepayment may vary considerably by the type of underlying asset.</fibo-fnd-utl-av:explanatoryNote>
	</owl:Class>
	
	<owl:Class rdf:about="&fibo-sec-dbt-ab-abs;HomeEquityLineOfCreditPool">
		<rdfs:subClassOf rdf:resource="&fibo-sec-dbt-ab-abs;LoanPool"/>
		<rdfs:subClassOf>
			<owl:Restriction>
				<owl:onProperty rdf:resource="&fibo-fnd-arr-arr;hasConstituent"/>
				<owl:someValuesFrom rdf:resource="&fibo-sec-dbt-ab-abs;HomeEquityLineOfCreditPoolConstituent"/>
			</owl:Restriction>
		</rdfs:subClassOf>
		<rdfs:label xml:lang="en">home equity line of credit pool</rdfs:label>
		<owl:disjointWith rdf:resource="&fibo-sec-dbt-ab-mbs;MortgagePool"/>
	</owl:Class>
	
	<owl:Class rdf:about="&fibo-sec-dbt-ab-abs;HomeEquityLineOfCreditPoolConstituent">
		<rdfs:subClassOf rdf:resource="&fibo-sec-dbt-ab-abs;LoanPoolConstituent"/>
		<rdfs:label xml:lang="en">home equity line of credit pool constituent</rdfs:label>
		<skos:definition xml:lang="en">A line of credit defined as a constituent of a Home Equity Line Of Credit Pool.</skos:definition>
	</owl:Class>
	
	<owl:Class rdf:about="&fibo-sec-dbt-ab-abs;IndexAmortizingBond">
		<rdfs:subClassOf rdf:resource="&fibo-sec-dbt-ab-abs;IndexBasedCouponBond"/>
		<rdfs:subClassOf rdf:resource="&fibo-sec-dbt-bnd;AmortizingBond"/>
		<rdfs:subClassOf>
			<owl:Restriction>
				<owl:onProperty rdf:resource="&fibo-sec-dbt-dbti;hasRepaymentTerms"/>
				<owl:someValuesFrom rdf:resource="&fibo-sec-dbt-ab-abs;IndexLinkedPrincipalDeterminationTerms"/>
			</owl:Restriction>
		</rdfs:subClassOf>
		<rdfs:label>index amortizing bond</rdfs:label>
		<skos:definition></skos:definition>
	</owl:Class>
	
	<owl:Class rdf:about="&fibo-sec-dbt-ab-abs;IndexBasedCouponBond">
		<rdfs:subClassOf rdf:resource="&fibo-sec-dbt-bnd;VariableCouponBond"/>
		<rdfs:subClassOf>
			<owl:Restriction>
				<owl:onProperty rdf:resource="&fibo-fbc-dae-dbt;hasInterestRate"/>
				<owl:someValuesFrom rdf:resource="&fibo-sec-dbt-ab-abs;IndexLinkedCoupon"/>
			</owl:Restriction>
		</rdfs:subClassOf>
		<rdfs:subClassOf>
			<owl:Restriction>
				<owl:onProperty rdf:resource="&fibo-sec-dbt-dbti;hasInterestPaymentTerms"/>
				<owl:someValuesFrom rdf:resource="&fibo-sec-dbt-ab-abs;IndexLinkedCouponTerms"/>
			</owl:Restriction>
		</rdfs:subClassOf>
		<rdfs:label>index-based coupon bond</rdfs:label>
		<skos:definition>variable coupon bond with payments that fluctuate according to an &quot;index&quot; other than an interest rate, such as an economic indicator</skos:definition>
		<skos:editorialNote>Might also be referred to as Index Linked, but more commonly the term Index Linked refers to principal. So this term has a made up name for this kind of bond, following OTPP review in which we dealt with the distinction between index linked interest and index linked principal amounts. .</skos:editorialNote>
	</owl:Class>
	
	<owl:Class rdf:about="&fibo-sec-dbt-ab-abs;IndexLinkedCoupon">
		<rdfs:subClassOf rdf:resource="&fibo-sec-dbt-bnd;BondVariableCoupon"/>
		<rdfs:label>index linked coupon</rdfs:label>
		<owl:disjointWith rdf:resource="&fibo-sec-dbt-ab-abs;InflationBondVariableCoupon"/>
		<owl:disjointWith rdf:resource="&fibo-sec-dbt-ab-abs;WACBondCoupon"/>
	</owl:Class>
	
	<owl:Class rdf:about="&fibo-sec-dbt-ab-abs;IndexLinkedCouponTerms">
		<rdfs:subClassOf rdf:resource="&fibo-sec-dbt-bnd;VariableCouponTerms"/>
		<rdfs:subClassOf>
			<owl:Restriction>
				<owl:onProperty rdf:resource="&fibo-fbc-dae-dbt;isBasedOn"/>
				<owl:someValuesFrom>
					<owl:Class>
						<owl:unionOf rdf:parseType="Collection">
							<rdf:Description rdf:about="&fibo-ind-ei-ei;EconomicIndicator">
							</rdf:Description>
							<rdf:Description rdf:about="&fibo-ind-ind-ind;MarketRate">
							</rdf:Description>
						</owl:unionOf>
					</owl:Class>
				</owl:someValuesFrom>
			</owl:Restriction>
		</rdfs:subClassOf>
		<rdfs:label>index-linked coupon terms</rdfs:label>
	</owl:Class>
	
	<owl:Class rdf:about="&fibo-sec-dbt-ab-abs;IndexLinkedPrincipalDeterminationTerms">
		<rdfs:subClassOf rdf:resource="&fibo-sec-dbt-dbti;TradableDebtInstrumentRedemptionProvision"/>
		<rdfs:subClassOf>
			<owl:Restriction>
				<owl:onProperty rdf:resource="&fibo-fnd-utl-alx;hasExpression"/>
				<owl:someValuesFrom rdf:resource="&fibo-sec-dbt-ab-abs;PrincipalPaymentCalculation"/>
			</owl:Restriction>
		</rdfs:subClassOf>
		<rdfs:subClassOf>
			<owl:Restriction>
				<owl:onProperty rdf:resource="&fibo-sec-dbt-ab-abs;specifiesIndexParameter"/>
				<owl:someValuesFrom>
					<owl:Class>
						<owl:unionOf rdf:parseType="Collection">
							<rdf:Description rdf:about="&fibo-ind-ei-ei;EconomicIndicator">
							</rdf:Description>
							<rdf:Description rdf:about="&fibo-ind-ind-ind;MarketRate">
							</rdf:Description>
						</owl:unionOf>
					</owl:Class>
				</owl:someValuesFrom>
			</owl:Restriction>
		</rdfs:subClassOf>
		<rdfs:label>index-linked principal determination terms</rdfs:label>
		<skos:definition>terms for payment of the principal that tie the principal amounts to some underlying index or interest rate</skos:definition>
	</owl:Class>
	
	<owl:Class rdf:about="&fibo-sec-dbt-ab-abs;InflationBondInterestPaymentTerms">
		<rdfs:subClassOf rdf:resource="&fibo-sec-dbt-bnd;CouponPaymentTerms"/>
		<rdfs:label>inflation bond interest payment terms</rdfs:label>
		<skos:definition>terms for the payment of interest on an inflation bond</skos:definition>
		<fibo-fnd-utl-av:explanatoryNote>These may for example specify that the interest payments are by way of coupone calculated with reference to the inflation rate that is referenced for that bond, or they may not (for example they may specify a fixed coupon amount). Therefore these terms may specify any potential interest payment arrangement used on bonds.</fibo-fnd-utl-av:explanatoryNote>
	</owl:Class>
	
	<owl:Class rdf:about="&fibo-sec-dbt-ab-abs;InflationBondPrincipalRepaymentTerms">
		<rdfs:subClassOf rdf:resource="&fibo-sec-dbt-ab-abs;IndexLinkedPrincipalDeterminationTerms"/>
		<rdfs:subClassOf>
			<owl:Restriction>
				<owl:onProperty rdf:resource="&fibo-fnd-utl-alx;hasExpression"/>
				<owl:someValuesFrom rdf:resource="&fibo-sec-dbt-ab-abs;InflationFactorExpression"/>
			</owl:Restriction>
		</rdfs:subClassOf>
		<rdfs:label>inflation bond principal repayment terms</rdfs:label>
		<skos:definition>terms specifying how the principal amount on an inflation bond is to be paid down</skos:definition>
		<fibo-fnd-utl-av:explanatoryNote>Further notes: This is typically but not necessarily with reference to the Inflation rate that is referred to for this bond. Further model action: identify and model terms for the case where the bond principal repayments are not pegged to an inflation rate.</fibo-fnd-utl-av:explanatoryNote>
	</owl:Class>
	
	<owl:Class rdf:about="&fibo-sec-dbt-ab-abs;InflationBondVariableCoupon">
		<rdfs:subClassOf rdf:resource="&fibo-sec-dbt-bnd;BondVariableCoupon"/>
		<rdfs:label>inflation bond variable coupon</rdfs:label>
		<owl:disjointWith rdf:resource="&fibo-sec-dbt-ab-abs;WACBondCoupon"/>
	</owl:Class>
	
	<owl:Class rdf:about="&fibo-sec-dbt-ab-abs;InflationBondVariableCouponTerms">
		<rdfs:subClassOf rdf:resource="&fibo-sec-dbt-bnd;VariableCouponTerms"/>
		<rdfs:subClassOf>
			<owl:Restriction>
				<owl:onProperty rdf:resource="&fibo-fbc-dae-dbt;hasInterestRate"/>
				<owl:onClass rdf:resource="&fibo-sec-dbt-ab-abs;InflationBondVariableCoupon"/>
				<owl:maxQualifiedCardinality rdf:datatype="&xsd;nonNegativeInteger">1</owl:maxQualifiedCardinality>
			</owl:Restriction>
		</rdfs:subClassOf>
		<rdfs:subClassOf>
			<owl:Restriction>
				<owl:onProperty rdf:resource="&fibo-fnd-utl-alx;hasExpression"/>
				<owl:someValuesFrom rdf:resource="&fibo-sec-dbt-ab-abs;InflationFactorExpression"/>
			</owl:Restriction>
		</rdfs:subClassOf>
		<rdfs:label>inflation bond variable coupon terms</rdfs:label>
	</owl:Class>
	
	<owl:Class rdf:about="&fibo-sec-dbt-ab-abs;InflationFactorExpression">
		<rdfs:subClassOf rdf:resource="&fibo-fnd-utl-alx;Expression"/>
		<rdfs:subClassOf>
			<owl:Restriction>
				<owl:onProperty rdf:resource="&fibo-fnd-utl-alx;hasArgument"/>
				<owl:someValuesFrom rdf:resource="&fibo-ind-ei-ei;InflationRate"/>
			</owl:Restriction>
		</rdfs:subClassOf>
		<rdfs:label>inflation factor expression</rdfs:label>
		<skos:definition>expression used to calculate the outstanding principal of the bond due to changes in the inflation rate</skos:definition>
	</owl:Class>
	
	<owl:Class rdf:about="&fibo-sec-dbt-ab-abs;LoanPool">
		<rdfs:subClassOf rdf:resource="&fibo-sec-dbt-ab-pbs;PoolOfIndividualDebts"/>
		<rdfs:subClassOf>
			<owl:Restriction>
				<owl:onProperty rdf:resource="&fibo-fnd-arr-arr;hasConstituent"/>
				<owl:someValuesFrom rdf:resource="&fibo-sec-dbt-ab-abs;LoanPoolConstituent"/>
			</owl:Restriction>
		</rdfs:subClassOf>
		<rdfs:label xml:lang="en">loan pool</rdfs:label>
		<skos:definition xml:lang="en">A number of loans, combined into a single pool and used as an asset.</skos:definition>
	</owl:Class>
	
	<owl:Class rdf:about="&fibo-sec-dbt-ab-abs;LoanPoolConstituent">
		<rdfs:subClassOf>
			<owl:Restriction>
				<owl:onProperty rdf:resource="&fibo-fnd-arr-arr;isConstituentOf"/>
				<owl:onClass rdf:resource="&fibo-sec-dbt-ab-abs;LoanPool"/>
				<owl:maxQualifiedCardinality rdf:datatype="&xsd;nonNegativeInteger">1</owl:maxQualifiedCardinality>
			</owl:Restriction>
		</rdfs:subClassOf>
		<rdfs:label xml:lang="en">loan pool constituent</rdfs:label>
		<skos:definition xml:lang="en">A loan constituent of a Loan Pool.</skos:definition>
	</owl:Class>
	
	<owl:Class rdf:about="&fibo-sec-dbt-ab-abs;PrincipalPaymentCalculation">
		<rdfs:subClassOf rdf:resource="&fibo-fnd-utl-alx;Expression"/>
		<rdfs:subClassOf>
			<owl:Restriction>
				<owl:onProperty rdf:resource="&fibo-fnd-utl-alx;hasArgument"/>
				<owl:someValuesFrom rdf:resource="&fibo-fbc-dae-dbt;Principal"/>
			</owl:Restriction>
		</rdfs:subClassOf>
		<rdfs:label>principal payment calculation</rdfs:label>
		<skos:definition>a formula for calculation of principal payments for certain kinds of bonds</skos:definition>
	</owl:Class>
	
	<owl:Class rdf:about="&fibo-sec-dbt-ab-abs;PromisedCashFlowAsset">
		<rdfs:subClassOf rdf:resource="&fibo-fnd-oac-own;Asset"/>
		<rdfs:label xml:lang="en">promised cash flow asset</rdfs:label>
		<skos:definition xml:lang="en">An asset which takes the form of some promised future cashflow. This may be securitized.</skos:definition>
		<fibo-fnd-utl-av:explanatoryNote xml:lang="en">For example, exotic Cash ABS instruments may be created where the underlying asset is not a pool of securities or debt but a promised cash flow. People have securitized the cash flows of businesses, artists, mobile phone tower income, airplane leases, lotto receivables, etc.</fibo-fnd-utl-av:explanatoryNote>
	</owl:Class>
	
	<owl:Class rdf:about="&fibo-sec-dbt-ab-abs;WACBondCoupon">
		<rdfs:subClassOf rdf:resource="&fibo-sec-dbt-bnd;BondVariableCoupon"/>
		<rdfs:label>w a c bond coupon</rdfs:label>
	</owl:Class>
	
	<owl:ObjectProperty rdf:about="&fibo-sec-dbt-ab-abs;balanceAtInclusionDate">
		<rdfs:label xml:lang="en">balance at inclusion date</rdfs:label>
		<rdfs:domain rdf:resource="&fibo-sec-dbt-ab-abs;LoanPoolConstituent"/>
		<rdfs:range rdf:resource="&fibo-fnd-acc-cur;MonetaryAmount"/>
	</owl:ObjectProperty>
	
	<owl:ObjectProperty rdf:about="&fibo-sec-dbt-ab-abs;category">
		<rdfs:label xml:lang="en">category</rdfs:label>
		<rdfs:domain rdf:resource="&fibo-sec-dbt-ab-abs;AutoLoanABS"/>
		<rdfs:range rdf:resource="&fibo-sec-dbt-ab-cdo;CreditworthinessSelection"/>
		<skos:definition xml:lang="en">Auto-loans ABS are classified into three categories: prime, non-prime, and sub-prime.</skos:definition>
	</owl:ObjectProperty>
	
	<owl:ObjectProperty rdf:about="&fibo-sec-dbt-ab-abs;definesTermsFor">
		<rdfs:label>defines terms for</rdfs:label>
	</owl:ObjectProperty>
	
	<owl:ObjectProperty rdf:about="&fibo-sec-dbt-ab-abs;describedAs">
		<rdfs:label xml:lang="en">described as</rdfs:label>
		<rdfs:domain rdf:resource="&fibo-sec-dbt-ab-abs;ABSIssuer"/>
		<rdfs:range rdf:resource="&fibo-sec-dbt-ab-spv;DebtSPV"/>
	</owl:ObjectProperty>
	
	<owl:DatatypeProperty rdf:about="&fibo-sec-dbt-ab-abs;description">
		<rdfs:label xml:lang="en">description</rdfs:label>
		<rdfs:domain rdf:resource="&fibo-sec-dbt-ab-abs;PromisedCashFlowAsset"/>
		<rdfs:range rdf:resource="&xsd;string"/>
		<skos:definition xml:lang="en">a textual description of the cash flow used as an asset.</skos:definition>
	</owl:DatatypeProperty>
	
	<owl:ObjectProperty rdf:about="&fibo-sec-dbt-ab-abs;hasUnderlyingAssets">
		<rdfs:label xml:lang="en">has underlying assets</rdfs:label>
		<rdfs:domain rdf:resource="&fibo-sec-dbt-ab-abs;CashAssetBackedSecurityInstrument"/>
		<rdfs:range>
			<owl:Class>
				<owl:unionOf rdf:parseType="Collection">
					<rdf:Description rdf:about="&fibo-sec-dbt-ab-abs;CreditCardPool">
					</rdf:Description>
					<rdf:Description rdf:about="&fibo-sec-dbt-ab-abs;HomeEquityLineOfCreditPool">
					</rdf:Description>
					<rdf:Description rdf:about="&fibo-sec-dbt-ab-abs;LoanPool">
					</rdf:Description>
				</owl:unionOf>
			</owl:Class>
		</rdfs:range>
		<skos:definition xml:lang="en">The ABS has an underlying pool asset which is either a loan pool or a credit card pool. This is actually defined as being any kind of pool asset that is not a mortgage pool, so any other types of pool should be added. This is more satisfactory that modeling it with a &quot;not&quot; relationship to Mortgage Pool, though that may be more correct.</skos:definition>
	</owl:ObjectProperty>
	
	<owl:ObjectProperty rdf:about="&fibo-sec-dbt-ab-abs;hasUnderlyingCashflow">
		<rdfs:subPropertyOf rdf:resource="&fibo-sec-dbt-ab-abs;hasUnderlyingAssets"/>
		<rdfs:label xml:lang="en">has underlying cashflow</rdfs:label>
		<rdfs:domain rdf:resource="&fibo-sec-dbt-ab-abs;EsotericABS"/>
		<rdfs:range rdf:resource="&fibo-sec-dbt-ab-abs;PromisedCashFlowAsset"/>
	</owl:ObjectProperty>
	
	<owl:ObjectProperty rdf:about="&fibo-sec-dbt-ab-abs;poolHasLoanType">
		<rdfs:label xml:lang="en">pool has loan type</rdfs:label>
		<rdfs:domain rdf:resource="&fibo-sec-dbt-ab-abs;LoanPool"/>
		<rdfs:range rdf:resource="&fibo-loan-typ-prod;LoanPurpose"/>
		<skos:definition xml:lang="en">The type of loans that make up the pool.</skos:definition>
	</owl:ObjectProperty>
	
	<owl:DatatypeProperty rdf:about="&fibo-sec-dbt-ab-abs;revolving">
		<rdfs:label xml:lang="en">revolving</rdfs:label>
		<rdfs:domain rdf:resource="&fibo-sec-dbt-ab-abs;CreditCardPool"/>
		<rdfs:domain rdf:resource="&fibo-sec-dbt-ab-abs;HomeEquityLineOfCreditPool"/>
		<rdfs:range rdf:resource="&xsd;boolean"/>
		<skos:definition xml:lang="en">Feature whereby the principal can go up or down. This means that the loan could pay down principal or add principal to it.</skos:definition>
	</owl:DatatypeProperty>
	
	<owl:ObjectProperty rdf:about="&fibo-sec-dbt-ab-abs;specifiesIndexParameter">
		<rdfs:label>specifies index parameter</rdfs:label>
		<rdfs:domain rdf:resource="&fibo-sec-dbt-ab-abs;IndexLinkedPrincipalDeterminationTerms"/>
		<rdfs:range rdf:resource="&fibo-ind-ei-ei;InflationRate"/>
		<skos:definition>indicates the index specified in the formula for determination of principal paydown amounts</skos:definition>
	</owl:ObjectProperty>
	
	<owl:ObjectProperty rdf:about="&fibo-sec-dbt-ab-abs;subordinatedTo">
		<rdfs:subPropertyOf rdf:resource="&fibo-sec-dbt-dbti;mayBeSubordinatedTo"/>
		<rdfs:label xml:lang="en">subordinated to</rdfs:label>
		<rdfs:domain rdf:resource="&fibo-sec-dbt-ab-abs;CashAssetBackedSecurityInstrument"/>
		<rdfs:range rdf:resource="&fibo-sec-dbt-ab-abs;CashAssetBackedSecurityInstrument"/>
	</owl:ObjectProperty>
	
	<owl:DatatypeProperty rdf:about="&fibo-sec-dbt-ab-abs;tranche">
		<rdfs:label xml:lang="en">tranche</rdfs:label>
		<rdfs:domain rdf:resource="&fibo-sec-dbt-ab-abs;CashAssetBackedSecurityInstrument"/>
		<rdfs:range rdf:resource="&xsd;string"/>
		<skos:definition xml:lang="en">Security Tranche that this ABS security forms part of.</skos:definition>
	</owl:DatatypeProperty>
	
	<owl:Class rdf:about="&fibo-sec-dbt-bnd;InflationBond">
		<rdfs:subClassOf>
			<owl:Restriction>
				<owl:onProperty rdf:resource="&fibo-sec-dbt-dbti;hasRepaymentTerms"/>
				<owl:onClass rdf:resource="&fibo-sec-dbt-ab-abs;IndexLinkedPrincipalDeterminationTerms"/>
				<owl:maxQualifiedCardinality rdf:datatype="&xsd;nonNegativeInteger">1</owl:maxQualifiedCardinality>
			</owl:Restriction>
		</rdfs:subClassOf>
		<rdfs:subClassOf>
			<owl:Restriction>
				<owl:onProperty rdf:resource="&fibo-sec-dbt-dbti;hasInterestPaymentTerms"/>
				<owl:someValuesFrom rdf:resource="&fibo-sec-dbt-ab-abs;InflationBondInterestPaymentTerms"/>
			</owl:Restriction>
		</rdfs:subClassOf>
		<rdfs:subClassOf>
			<owl:Restriction>
				<owl:onProperty rdf:resource="&fibo-sec-dbt-dbti;hasInterestPaymentTerms"/>
				<owl:someValuesFrom rdf:resource="&fibo-sec-dbt-ab-abs;InflationBondVariableCouponTerms"/>
			</owl:Restriction>
		</rdfs:subClassOf>
		<rdfs:subClassOf>
			<owl:Restriction>
				<owl:onProperty rdf:resource="&fibo-sec-dbt-dbti;hasRepaymentTerms"/>
				<owl:someValuesFrom rdf:resource="&fibo-sec-dbt-ab-abs;InflationBondPrincipalRepaymentTerms"/>
			</owl:Restriction>
		</rdfs:subClassOf>
		<fibo-fnd-utl-av:explanatoryNote>The inflation rate is used to define the factor or multiplier for the bond, that is the factor that you multiply the bond by. How this works is that you take the inflation rate when the security was issued, and the inflation rate at the present. The difference between these becomes the Factor, e.g. 100% -&amp;gt; 101% gives 1% so for example for a $1000 issue - calculate the principal on which the interest is paid AND the principal from the point of view of how the principal is repaid. Some inflation bonds only do this on interest, some only on interest, but most apply it to the principal and interest. Coupon interest calculated based on the adjusted amount of the bond. so a fixed coupon rate is multiplied by e.g. 1010 in the example above. Variations e.g. Italy - daily published factor published for that bond, whereas other calculate based on underlying index. Typically a CPI or a statistical number generated by the govt. typically a lagging three month index. See UK bonds on this. US and Japanese ones - look at inflation rate 3 months prior. Unlike an Amortizing Security this principal value of the bond is increasing, whereas for and Amortizing, the principal is decreasing. In Canada, these are also referred to as &quot;real return bonds&quot;. 
Further Notes:Additional review with OTPP May 05 2010 indicates that this is part of a classification of bonds where the principal amount itself varies according to some index, a point which was not understood at the original review session. Terms and labels revised to fit this picture.</fibo-fnd-utl-av:explanatoryNote>
	</owl:Class>

</rdf:RDF>