<?xml version="1.0" encoding="UTF-8"?>
<!DOCTYPE rdf:RDF [
	<!ENTITY dct "http://purl.org/dc/terms/">
	<!ENTITY fibo-be-fct-fct "https://spec.edmcouncil.org/fibo/ontology/BE/FunctionalEntities/FunctionalEntities/">
	<!ENTITY fibo-be-le-lp "https://spec.edmcouncil.org/fibo/ontology/BE/LegalEntities/LegalPersons/">
	<!ENTITY fibo-bp-iss-dbti "https://spec.edmcouncil.org/fibo/ontology/BP/SecuritiesIssuance/DebtIssuance/">
	<!ENTITY fibo-bp-iss-trm "https://spec.edmcouncil.org/fibo/ontology/BP/SecuritiesIssuance/IssuanceProcessTerms/">
	<!ENTITY fibo-fbc-dae-dbt "https://spec.edmcouncil.org/fibo/ontology/FBC/DebtAndEquities/Debt/">
	<!ENTITY fibo-fbc-fct-fse "https://spec.edmcouncil.org/fibo/ontology/FBC/FunctionalEntities/FinancialServicesEntities/">
	<!ENTITY fibo-fnd-acc-cur "https://spec.edmcouncil.org/fibo/ontology/FND/Accounting/CurrencyAmount/">
	<!ENTITY fibo-fnd-arr-arr "https://spec.edmcouncil.org/fibo/ontology/FND/Arrangements/Arrangements/">
	<!ENTITY fibo-fnd-dt-bd "https://spec.edmcouncil.org/fibo/ontology/FND/DatesAndTimes/BusinessDates/">
	<!ENTITY fibo-fnd-dt-fd "https://spec.edmcouncil.org/fibo/ontology/FND/DatesAndTimes/FinancialDates/">
	<!ENTITY fibo-fnd-pas-psch "https://spec.edmcouncil.org/fibo/ontology/FND/ProductsAndServices/PaymentsAndSchedules/">
	<!ENTITY fibo-fnd-pty-pty "https://spec.edmcouncil.org/fibo/ontology/FND/Parties/Parties/">
	<!ENTITY fibo-fnd-rel-rel "https://spec.edmcouncil.org/fibo/ontology/FND/Relations/Relations/">
	<!ENTITY fibo-fnd-utl-av "https://spec.edmcouncil.org/fibo/ontology/FND/Utilities/AnnotationVocabulary/">
	<!ENTITY fibo-fnd-utl-val "https://spec.edmcouncil.org/fibo/ontology/FND/Utilities/Values/">
	<!ENTITY fibo-loan-tem-ev "https://spec.edmcouncil.org/fibo/ontology/LOAN/LoansTemporal/LoansEvents/">
	<!ENTITY fibo-md-dbtx-aly "https://spec.edmcouncil.org/fibo/ontology/MD/DebtTemporal/DebtAnalytics/">
	<!ENTITY fibo-sec-dbt-ab-abs "https://spec.edmcouncil.org/fibo/ontology/SEC/Debt/AssetBackedSecurities/AssetBackedSecurities/">
	<!ENTITY fibo-sec-dbt-ab-cmo "https://spec.edmcouncil.org/fibo/ontology/SEC/Debt/AssetBackedSecurities/CMOs/">
	<!ENTITY fibo-sec-dbt-ab-mbs "https://spec.edmcouncil.org/fibo/ontology/SEC/Debt/AssetBackedSecurities/MortgageBackedSecurities/">
	<!ENTITY fibo-sec-dbt-ab-pbs "https://spec.edmcouncil.org/fibo/ontology/SEC/Debt/AssetBackedSecurities/PoolBackedSecurities/">
	<!ENTITY fibo-sec-dbt-dbti "https://spec.edmcouncil.org/fibo/ontology/SEC/Debt/DebtInstruments/">
	<!ENTITY fibo-sec-sec-iss "https://spec.edmcouncil.org/fibo/ontology/SEC/Securities/SecuritiesIssuance/">
	<!ENTITY owl "http://www.w3.org/2002/07/owl#">
	<!ENTITY rdf "http://www.w3.org/1999/02/22-rdf-syntax-ns#">
	<!ENTITY rdfs "http://www.w3.org/2000/01/rdf-schema#">
	<!ENTITY skos "http://www.w3.org/2004/02/skos/core#">
	<!ENTITY xsd "http://www.w3.org/2001/XMLSchema#">
]>
<rdf:RDF xml:base="https://spec.edmcouncil.org/fibo/ontology/SEC/Debt/AssetBackedSecurities/MortgageBackedSecurities/"
	xmlns:dct="http://purl.org/dc/terms/"
	xmlns:fibo-be-fct-fct="https://spec.edmcouncil.org/fibo/ontology/BE/FunctionalEntities/FunctionalEntities/"
	xmlns:fibo-be-le-lp="https://spec.edmcouncil.org/fibo/ontology/BE/LegalEntities/LegalPersons/"
	xmlns:fibo-bp-iss-dbti="https://spec.edmcouncil.org/fibo/ontology/BP/SecuritiesIssuance/DebtIssuance/"
	xmlns:fibo-bp-iss-trm="https://spec.edmcouncil.org/fibo/ontology/BP/SecuritiesIssuance/IssuanceProcessTerms/"
	xmlns:fibo-fbc-dae-dbt="https://spec.edmcouncil.org/fibo/ontology/FBC/DebtAndEquities/Debt/"
	xmlns:fibo-fbc-fct-fse="https://spec.edmcouncil.org/fibo/ontology/FBC/FunctionalEntities/FinancialServicesEntities/"
	xmlns:fibo-fnd-acc-cur="https://spec.edmcouncil.org/fibo/ontology/FND/Accounting/CurrencyAmount/"
	xmlns:fibo-fnd-arr-arr="https://spec.edmcouncil.org/fibo/ontology/FND/Arrangements/Arrangements/"
	xmlns:fibo-fnd-dt-bd="https://spec.edmcouncil.org/fibo/ontology/FND/DatesAndTimes/BusinessDates/"
	xmlns:fibo-fnd-dt-fd="https://spec.edmcouncil.org/fibo/ontology/FND/DatesAndTimes/FinancialDates/"
	xmlns:fibo-fnd-pas-psch="https://spec.edmcouncil.org/fibo/ontology/FND/ProductsAndServices/PaymentsAndSchedules/"
	xmlns:fibo-fnd-pty-pty="https://spec.edmcouncil.org/fibo/ontology/FND/Parties/Parties/"
	xmlns:fibo-fnd-rel-rel="https://spec.edmcouncil.org/fibo/ontology/FND/Relations/Relations/"
	xmlns:fibo-fnd-utl-av="https://spec.edmcouncil.org/fibo/ontology/FND/Utilities/AnnotationVocabulary/"
	xmlns:fibo-fnd-utl-val="https://spec.edmcouncil.org/fibo/ontology/FND/Utilities/Values/"
	xmlns:fibo-loan-tem-ev="https://spec.edmcouncil.org/fibo/ontology/LOAN/LoansTemporal/LoansEvents/"
	xmlns:fibo-md-dbtx-aly="https://spec.edmcouncil.org/fibo/ontology/MD/DebtTemporal/DebtAnalytics/"
	xmlns:fibo-sec-dbt-ab-abs="https://spec.edmcouncil.org/fibo/ontology/SEC/Debt/AssetBackedSecurities/AssetBackedSecurities/"
	xmlns:fibo-sec-dbt-ab-cmo="https://spec.edmcouncil.org/fibo/ontology/SEC/Debt/AssetBackedSecurities/CMOs/"
	xmlns:fibo-sec-dbt-ab-mbs="https://spec.edmcouncil.org/fibo/ontology/SEC/Debt/AssetBackedSecurities/MortgageBackedSecurities/"
	xmlns:fibo-sec-dbt-ab-pbs="https://spec.edmcouncil.org/fibo/ontology/SEC/Debt/AssetBackedSecurities/PoolBackedSecurities/"
	xmlns:fibo-sec-dbt-dbti="https://spec.edmcouncil.org/fibo/ontology/SEC/Debt/DebtInstruments/"
	xmlns:fibo-sec-sec-iss="https://spec.edmcouncil.org/fibo/ontology/SEC/Securities/SecuritiesIssuance/"
	xmlns:owl="http://www.w3.org/2002/07/owl#"
	xmlns:rdf="http://www.w3.org/1999/02/22-rdf-syntax-ns#"
	xmlns:rdfs="http://www.w3.org/2000/01/rdf-schema#"
	xmlns:skos="http://www.w3.org/2004/02/skos/core#"
	xmlns:xsd="http://www.w3.org/2001/XMLSchema#">
	
	<owl:Ontology rdf:about="https://spec.edmcouncil.org/fibo/ontology/SEC/Debt/AssetBackedSecurities/MortgageBackedSecurities/">
		<rdfs:label xml:lang="en">MortgageBackedSecurities</rdfs:label>
		<dct:abstract>Mortgage backed securities are like asset backed securities except that the underlying loan pool is a pool of mortgage loans.</dct:abstract>
		<owl:imports rdf:resource="https://spec.edmcouncil.org/fibo/ontology/BE/FunctionalEntities/FunctionalEntities/"/>
		<owl:imports rdf:resource="https://spec.edmcouncil.org/fibo/ontology/BE/LegalEntities/LegalPersons/"/>
		<owl:imports rdf:resource="https://spec.edmcouncil.org/fibo/ontology/BP/SecuritiesIssuance/DebtIssuance/"/>
		<owl:imports rdf:resource="https://spec.edmcouncil.org/fibo/ontology/BP/SecuritiesIssuance/IssuanceProcessTerms/"/>
		<owl:imports rdf:resource="https://spec.edmcouncil.org/fibo/ontology/FBC/DebtAndEquities/Debt/"/>
		<owl:imports rdf:resource="https://spec.edmcouncil.org/fibo/ontology/FBC/FunctionalEntities/FinancialServicesEntities/"/>
		<owl:imports rdf:resource="https://spec.edmcouncil.org/fibo/ontology/FND/Accounting/CurrencyAmount/"/>
		<owl:imports rdf:resource="https://spec.edmcouncil.org/fibo/ontology/FND/DatesAndTimes/BusinessDates/"/>
		<owl:imports rdf:resource="https://spec.edmcouncil.org/fibo/ontology/FND/DatesAndTimes/FinancialDates/"/>
		<owl:imports rdf:resource="https://spec.edmcouncil.org/fibo/ontology/FND/Parties/Parties/"/>
		<owl:imports rdf:resource="https://spec.edmcouncil.org/fibo/ontology/FND/ProductsAndServices/PaymentsAndSchedules/"/>
		<owl:imports rdf:resource="https://spec.edmcouncil.org/fibo/ontology/FND/Relations/Relations/"/>
		<owl:imports rdf:resource="https://spec.edmcouncil.org/fibo/ontology/FND/Utilities/AnnotationVocabulary/"/>
		<owl:imports rdf:resource="https://spec.edmcouncil.org/fibo/ontology/FND/Utilities/Values/"/>
		<owl:imports rdf:resource="https://spec.edmcouncil.org/fibo/ontology/LOAN/LoansTemporal/LoansEvents/"/>
		<owl:imports rdf:resource="https://spec.edmcouncil.org/fibo/ontology/MD/DebtTemporal/DebtAnalytics/"/>
		<owl:imports rdf:resource="https://spec.edmcouncil.org/fibo/ontology/SEC/Debt/AssetBackedSecurities/AssetBackedSecurities/"/>
		<owl:imports rdf:resource="https://spec.edmcouncil.org/fibo/ontology/SEC/Debt/AssetBackedSecurities/CDOs/"/>
		<owl:imports rdf:resource="https://spec.edmcouncil.org/fibo/ontology/SEC/Debt/AssetBackedSecurities/CMOs/"/>
		<owl:imports rdf:resource="https://spec.edmcouncil.org/fibo/ontology/SEC/Debt/AssetBackedSecurities/PoolBackedSecurities/"/>
		<owl:imports rdf:resource="https://spec.edmcouncil.org/fibo/ontology/SEC/Debt/DebtInstruments/"/>
		<owl:imports rdf:resource="https://spec.edmcouncil.org/fibo/ontology/SEC/Securities/SecuritiesIssuance/"/>
		<owl:versionIRI rdf:resource="https://spec.edmcouncil.org/fibo/ontology/SEC/Debt/AssetBackedSecurities/MortgageBackedSecurities/"/>
		<fibo-fnd-utl-av:hasMaturityLevel rdf:resource="&fibo-fnd-utl-av;Provisional"/>
	</owl:Ontology>
	
	<owl:Class rdf:about="&fibo-sec-dbt-ab-mbs;AgencyMBSDeal">
		<rdfs:subClassOf rdf:resource="&fibo-sec-dbt-ab-mbs;MBSDeal"/>
		<rdfs:label xml:lang="en">agency m b s deal</rdfs:label>
		<owl:disjointWith rdf:resource="&fibo-sec-dbt-ab-mbs;PrivateLabelMBSDeal"/>
		<skos:definition xml:lang="en">An issue of securities backed by pools of mortgages held by government agencies.</skos:definition>
		<fibo-fnd-utl-av:explanatoryNote xml:lang="en">These are Ginnie Mae, Freddie Mac and Fannie Mae (for the US). Of these agencies, GNMA (Ginnie Mae) issues mortgages in its own right (Investorwords differs on this). Fannie Mae and Freddie Mac purchase mortgages. Those mortgages are issued by banks. Before one of these agencies purchases a mortgage, there are certain criteria that have to be met. These are specified in terms of, for example, the balance of the mortgage, limits to credit ratings.</fibo-fnd-utl-av:explanatoryNote>
	</owl:Class>
	
	<owl:Class rdf:about="&fibo-sec-dbt-ab-mbs;AgencyMBSIssuer">
		<rdfs:subClassOf rdf:resource="&fibo-sec-dbt-ab-mbs;GovernmentMortgageAgency"/>
		<rdfs:subClassOf rdf:resource="&fibo-sec-dbt-ab-mbs;MBSIssuer"/>
		<rdfs:label xml:lang="en">agency m b s issuer</rdfs:label>
		<skos:definition xml:lang="en">The issuer of the pass through MBS is an Agency issuer. This is identified as being some kind of agency that is set up specifically to issue these instruments.</skos:definition>
	</owl:Class>
	
	<owl:Class rdf:about="&fibo-sec-dbt-ab-mbs;AgencyMBSPool">
		<rdfs:subClassOf rdf:resource="&fibo-sec-dbt-ab-mbs;MBSPool"/>
		<rdfs:label xml:lang="en">agency m b s pool</rdfs:label>
		<skos:definition xml:lang="en">A pool investment consisting of a collection of Agency MBS instruments.</skos:definition>
		<fibo-fnd-utl-av:explanatoryNote xml:lang="en">This pool may be used as the underlying for an agency CMO. Non agency CMOs do not exist.</fibo-fnd-utl-av:explanatoryNote>
	</owl:Class>
	
	<owl:Class rdf:about="&fibo-sec-dbt-ab-mbs;AgencyMortgagePool">
		<rdfs:subClassOf rdf:resource="&fibo-sec-dbt-ab-mbs;MortgagePool"/>
		<rdfs:label xml:lang="en">agency mortgage pool</rdfs:label>
		<owl:disjointWith rdf:resource="&fibo-sec-dbt-ab-mbs;NonAgencyMortgagePool"/>
		<skos:definition xml:lang="en">A pool of agency mortgages.</skos:definition>
	</owl:Class>
	
	<owl:Class rdf:about="&fibo-sec-dbt-ab-mbs;CommercialMBS">
		<rdfs:subClassOf rdf:resource="&fibo-sec-dbt-ab-mbs;MortgageBackedSecurityInstrument"/>
		<rdfs:label xml:lang="en">commercial m b s</rdfs:label>
		<owl:disjointWith rdf:resource="&fibo-sec-dbt-ab-mbs;ResidentialMBS"/>
	</owl:Class>
	
	<owl:Class rdf:about="&fibo-sec-dbt-ab-mbs;FHLMC-GoldPool">
		<rdfs:subClassOf rdf:resource="&fibo-sec-dbt-ab-mbs;AgencyMortgagePool"/>
		<rdfs:label xml:lang="en">FHLMC Gold pool</rdfs:label>
	</owl:Class>
	
	<owl:Class rdf:about="&fibo-sec-dbt-ab-mbs;FHLMC-Pool">
		<rdfs:subClassOf rdf:resource="&fibo-sec-dbt-ab-mbs;AgencyMortgagePool"/>
		<rdfs:label xml:lang="en">FHLMC pool</rdfs:label>
	</owl:Class>
	
	<owl:Class rdf:about="&fibo-sec-dbt-ab-mbs;FNMA-Pool">
		<rdfs:subClassOf rdf:resource="&fibo-sec-dbt-ab-mbs;AgencyMortgagePool"/>
		<rdfs:label xml:lang="en">FNMA pool</rdfs:label>
	</owl:Class>
	
	<owl:Class rdf:about="&fibo-sec-dbt-ab-mbs;FloaterTranche">
		<rdfs:subClassOf rdf:resource="&fibo-sec-dbt-ab-mbs;TranchedMBSInstrument"/>
		<rdfs:subClassOf>
			<owl:Restriction>
				<owl:onProperty rdf:resource="&fibo-fnd-dt-fd;hasRecurrenceInterval"/>
				<owl:someValuesFrom rdf:resource="&fibo-fnd-dt-bd;DayOfMonth"/>
			</owl:Restriction>
		</rdfs:subClassOf>
		<rdfs:label xml:lang="en">floater tranche</rdfs:label>
		<skos:definition xml:lang="en">A floater tranche is a tranche that is keyed to an index and a spread.</skos:definition>
		<fibo-fnd-utl-av:explanatoryNote xml:lang="en">For example, 3 month LIBOR +50 -- meaning that the coupon would be whatever the 3 month LIBOR is plus 50 basis points. This is not a continuously updated number, rather it resets at specified intervals.</fibo-fnd-utl-av:explanatoryNote>
	</owl:Class>
	
	<owl:Class rdf:about="&fibo-sec-dbt-ab-mbs;GNMA-IIPool">
		<rdfs:subClassOf rdf:resource="&fibo-sec-dbt-ab-mbs;AgencyMortgagePool"/>
		<rdfs:label xml:lang="en">GNMA-II pool</rdfs:label>
	</owl:Class>
	
	<owl:Class rdf:about="&fibo-sec-dbt-ab-mbs;GNMA-PlatinumPool">
		<rdfs:subClassOf rdf:resource="&fibo-sec-dbt-ab-mbs;AgencyMortgagePool"/>
		<rdfs:label xml:lang="en">GNMA Platinum pool</rdfs:label>
	</owl:Class>
	
	<owl:Class rdf:about="&fibo-sec-dbt-ab-mbs;GNMA-iPool">
		<rdfs:subClassOf rdf:resource="&fibo-sec-dbt-ab-mbs;AgencyMortgagePool"/>
		<rdfs:label xml:lang="en">GNMA-i pool</rdfs:label>
	</owl:Class>
	
	<owl:Class rdf:about="&fibo-sec-dbt-ab-mbs;GovernmentMortgageAgency">
		<rdfs:subClassOf rdf:resource="&fibo-be-fct-fct;FunctionalEntity"/>
		<rdfs:subClassOf>
			<owl:Restriction>
				<owl:onProperty rdf:resource="&fibo-fnd-rel-rel;hasIdentity"/>
				<owl:someValuesFrom rdf:resource="&fibo-be-le-lp;LegalEntity"/>
			</owl:Restriction>
		</rdfs:subClassOf>
		<rdfs:label xml:lang="en">government mortgage agency</rdfs:label>
		<skos:definition xml:lang="en">An agency set up by a government for the purpose of issuing mortgages.</skos:definition>
		<skos:editorialNote xml:lang="en">Note on the original property &apos;takes form of&apos;  (replaced by a restriction): The form which the Government Mortgage Agency takes. This is a Legal Entity and not a Natural Person, that is, it is an Artificial Person.</skos:editorialNote>
		<skos:scopeNote xml:lang="en">These exist in the USA and may also exist now or in future in other countries. There are three such agencies in thr USA: FNMA, GNMA and FHLMC (Fannie Mae, Ginnie Mae and Freddie Mac respectively).</skos:scopeNote>
	</owl:Class>
	
	<owl:Class rdf:about="&fibo-sec-dbt-ab-mbs;InverseFloaterTranche">
		<rdfs:subClassOf rdf:resource="&fibo-sec-dbt-ab-mbs;FloaterTranche"/>
		<rdfs:label xml:lang="en">inverse floater tranche</rdfs:label>
		<owl:disjointWith rdf:resource="&fibo-sec-dbt-ab-mbs;RegularFloaterTranche"/>
		<owl:disjointWith rdf:resource="&fibo-sec-dbt-ab-mbs;SuperFloaterTranche"/>
	</owl:Class>
	
	<owl:Class rdf:about="&fibo-sec-dbt-ab-mbs;IssuedAndSecuritizedAgencyMortagePool">
		<rdfs:subClassOf rdf:resource="&fibo-sec-dbt-ab-mbs;AgencyMortgagePool"/>
		<rdfs:subClassOf>
			<owl:Restriction>
				<owl:onProperty rdf:resource="&fibo-sec-dbt-ab-pbs;lifecycleState"/>
				<owl:someValuesFrom rdf:resource="&fibo-bp-iss-dbti;Issued"/>
			</owl:Restriction>
		</rdfs:subClassOf>
		<rdfs:label xml:lang="en">issued and securitized agency mortage pool</rdfs:label>
		<skos:definition xml:lang="en">An agency mortgage pool which has been securitized as part of an agency Mortgage Backed Security.</skos:definition>
	</owl:Class>
	
	<owl:Class rdf:about="&fibo-sec-dbt-ab-mbs;IssuedAndSecuritizedNonAgencyMortgagePool">
		<rdfs:subClassOf rdf:resource="&fibo-sec-dbt-ab-mbs;NonAgencyMortgagePool"/>
		<rdfs:subClassOf>
			<owl:Restriction>
				<owl:onProperty rdf:resource="&fibo-sec-dbt-ab-pbs;lifecycleState"/>
				<owl:someValuesFrom rdf:resource="&fibo-bp-iss-dbti;Issued"/>
			</owl:Restriction>
		</rdfs:subClassOf>
		<rdfs:label xml:lang="en">issued and securitized non agency mortgage pool</rdfs:label>
		<skos:definition xml:lang="en">A non agency mortgage pool which has been securitized as part of a tranched Mortgage Backed Security.</skos:definition>
	</owl:Class>
	
	<owl:Class rdf:about="&fibo-sec-dbt-ab-mbs;IssuedAndSecuritizedPoolOfIndividualDebts">
		<rdfs:subClassOf rdf:resource="&fibo-sec-dbt-ab-pbs;PoolOfIndividualDebts"/>
		<rdfs:subClassOf>
			<owl:Restriction>
				<owl:onProperty rdf:resource="&fibo-sec-dbt-ab-pbs;lifecycleState"/>
				<owl:someValuesFrom rdf:resource="&fibo-bp-iss-dbti;Issued"/>
			</owl:Restriction>
		</rdfs:subClassOf>
		<rdfs:label xml:lang="en">issued and securitized pool of individual debts</rdfs:label>
		<skos:definition xml:lang="en">A pool of individual debts (such as loans or mortgages) which is securitized as part of the issue of some security.</skos:definition>
	</owl:Class>
	
	<owl:Class rdf:about="&fibo-sec-dbt-ab-mbs;MBSDeal">
		<rdfs:subClassOf rdf:resource="&fibo-sec-dbt-ab-pbs;PoolBackedSecuritiesDeal"/>
		<rdfs:subClassOf>
			<owl:Restriction>
				<owl:onProperty rdf:resource="&fibo-sec-dbt-ab-pbs;hasUnderlying"/>
				<owl:someValuesFrom rdf:resource="&fibo-sec-dbt-ab-mbs;SecuritizedMortgagePool"/>
			</owl:Restriction>
		</rdfs:subClassOf>
		<rdfs:label xml:lang="en">m b s deal</rdfs:label>
		<skos:definition xml:lang="en">The issue of a series of Mortgage Backed Security certificates.</skos:definition>
	</owl:Class>
	
	<owl:Class rdf:about="&fibo-sec-dbt-ab-mbs;MBSDealProspectus">
		<rdfs:subClassOf rdf:resource="&fibo-sec-dbt-ab-pbs;PoolBackedDealProspectus"/>
		<rdfs:label xml:lang="en">m b s deal prospectus</rdfs:label>
		<skos:definition xml:lang="en">Prospectus describing the terms of the issue and each of the instruments included in the mortgage backed security issue. Term origin:SMER</skos:definition>
	</owl:Class>
	
	<owl:Class rdf:about="&fibo-sec-dbt-ab-mbs;MBSIssuer">
		<rdfs:subClassOf rdf:resource="&fibo-sec-dbt-ab-pbs;PoolBackedSecurityIssuer"/>
		<rdfs:subClassOf>
			<owl:Class>
				<owl:unionOf rdf:parseType="Collection">
					<rdf:Description rdf:about="&fibo-sec-dbt-ab-mbs;GovernmentMortgageAgency">
					</rdf:Description>
					<rdf:Description rdf:about="&fibo-fbc-fct-fse;Bank">
					</rdf:Description>
					<rdf:Description rdf:about="&fibo-sec-dbt-ab-mbs;SpecialistMortgageIssuer">
					</rdf:Description>
				</owl:unionOf>
			</owl:Class>
		</rdfs:subClassOf>
		<rdfs:label xml:lang="en">m b s issuer</rdfs:label>
		<skos:definition xml:lang="en">The issuer of a Mortgage Backed Security.</skos:definition>
		<fibo-fnd-utl-av:explanatoryNote xml:lang="en">This can be an agency that exists for this purpose or it may be the issuer of the original mortgages in the pool.</fibo-fnd-utl-av:explanatoryNote>
	</owl:Class>
	
	<owl:Class rdf:about="&fibo-sec-dbt-ab-mbs;MBSPool">
		<rdfs:subClassOf rdf:resource="&fibo-sec-dbt-ab-pbs;CashStructuredFinanceInstrumentPool"/>
		<rdfs:label xml:lang="en">m b s pool</rdfs:label>
		<skos:definition xml:lang="en">A pool investment consisting of a collection of MBS instruments.</skos:definition>
	</owl:Class>
	
	<owl:Class rdf:about="&fibo-sec-dbt-ab-mbs;MBSTrancheNote">
		<rdfs:subClassOf rdf:resource="&fibo-sec-dbt-ab-mbs;SecurityNote"/>
		<rdfs:label xml:lang="en">m b s tranche note</rdfs:label>
		<skos:definition xml:lang="en">An individual note of a tranche.</skos:definition>
		<fibo-fnd-utl-av:explanatoryNote xml:lang="en">A Tranche is made up of e.g. $500m in notes and so on. These may be in different notes, with different denominations. Analytics that would apply to the Tranche would by implication apply to each slice of the tranche.</fibo-fnd-utl-av:explanatoryNote>
	</owl:Class>
	
	<owl:Class rdf:about="&fibo-sec-dbt-ab-mbs;MezzanineMBSTranche">
		<rdfs:subClassOf rdf:resource="&fibo-sec-dbt-ab-mbs;TranchedMBSInstrument"/>
		<rdfs:subClassOf>
			<owl:Restriction>
				<owl:onProperty rdf:resource="&fibo-sec-dbt-ab-mbs;seniorTo"/>
				<owl:someValuesFrom rdf:resource="&fibo-sec-dbt-ab-mbs;SubordinatedMBSTranche"/>
			</owl:Restriction>
		</rdfs:subClassOf>
		<rdfs:label xml:lang="en">mezzanine m b s tranche</rdfs:label>
		<skos:definition xml:lang="en">Specific kinds of tranche are modeled for example and investigation only and have been removed from the diagrams. These will be removed from the final model.</skos:definition>
	</owl:Class>
	
	<owl:Class rdf:about="&fibo-sec-dbt-ab-mbs;MortgageBackedSecurityInstrument">
		<rdfs:subClassOf rdf:resource="&fibo-sec-dbt-ab-pbs;PoolBackedSecurityInstrument"/>
		<rdfs:subClassOf>
			<owl:Restriction>
				<owl:onProperty rdf:resource="&fibo-fnd-rel-rel;isCharacterizedBy"/>
				<owl:someValuesFrom rdf:resource="&fibo-md-dbtx-aly;MortgageInstrumentWeightedAverageRemainingMaturity"/>
			</owl:Restriction>
		</rdfs:subClassOf>
		<rdfs:subClassOf>
			<owl:Restriction>
				<owl:onProperty rdf:resource="&fibo-sec-dbt-ab-abs;definesTermsFor"/>
				<owl:someValuesFrom rdf:resource="&fibo-sec-dbt-ab-mbs;MortgageDebt"/>
			</owl:Restriction>
		</rdfs:subClassOf>
		<rdfs:subClassOf>
			<owl:Restriction>
				<owl:onProperty rdf:resource="&fibo-sec-dbt-ab-pbs;issuedBy"/>
				<owl:someValuesFrom rdf:resource="&fibo-sec-dbt-ab-mbs;MBSIssuer"/>
			</owl:Restriction>
		</rdfs:subClassOf>
		<rdfs:label xml:lang="en">mortgage backed security instrument</rdfs:label>
	</owl:Class>
	
	<owl:Class rdf:about="&fibo-sec-dbt-ab-mbs;MortgageCollateral">
		<rdfs:subClassOf rdf:resource="&fibo-fbc-dae-dbt;Collateral"/>
		<rdfs:label xml:lang="en">mortgage collateral</rdfs:label>
		<skos:definition xml:lang="en">Mortgage Debt Assets pledged to a lender until a loan is repaid. Further notes: This provides one means by which some extension of finance (such as a loan, debt or equity issue) is under-written.</skos:definition>
	</owl:Class>
	
	<owl:Class rdf:about="&fibo-sec-dbt-ab-mbs;MortgageDebt">
		<rdfs:subClassOf rdf:resource="&fibo-sec-dbt-ab-pbs;CollateralizedDebt"/>
		<rdfs:label xml:lang="en">mortgage debt</rdfs:label>
		<skos:definition xml:lang="en">Mortgage debt issued under a Mortgage Backed Security.</skos:definition>
	</owl:Class>
	
	<owl:Class rdf:about="&fibo-sec-dbt-ab-mbs;MortgagePool">
		<rdfs:subClassOf rdf:resource="&fibo-sec-dbt-ab-abs;LoanPool"/>
		<rdfs:subClassOf>
			<owl:Restriction>
				<owl:onProperty rdf:resource="&fibo-fnd-arr-arr;hasConstituent"/>
				<owl:someValuesFrom rdf:resource="&fibo-sec-dbt-ab-mbs;MortgagePoolConstituent"/>
			</owl:Restriction>
		</rdfs:subClassOf>
		<rdfs:label xml:lang="en">mortgage pool</rdfs:label>
		<skos:definition xml:lang="en">A number of mortgages combined into a single pool and used as an asset.</skos:definition>
		<skos:editorialNote xml:lang="en">Analytics review session notes: Dated facts (for non agency mortgage pools): Aggregate of : Scheduled payments (% and $) Payments Prepayments (% and $ notional) Default amounts (statistics: Prepayments: (start at 0 and ramp up and then level off (why?)) SMM basic measure monthly Basis CPR C? Prepayment Rate based on SMM annualised PSA based on CPR takes the COR and applies a curve to the rate of prepayments on the model. (%) e.g. 100% PSA is applied to model. 200% PSA implies x%CPR per month Tries to reflect how prepayments in a pool will accelerate and then burn out. This reflects the nature of a mortgage pool, elgl why people will prepay, refinance, address selection and so on i.e. local economy facts. so those will drop out of the pool and you are left with those who will not. that&apos;s why it levels off. So who originates these figures? Is it measured ongoing?: No . Used to determine a pricing speed when marketing the security to investors. So this is part of the primary market / issuance where there is marketing. These are the estimated figures as they will be at issue. PSA may also be used as triggers. 100 - 400% PSA band - if you go outside that band, may change payment behaviour of those classes. Defaults: measures or rate of default CDR conditional default rate (annual) MDR Monhtly default rate - like CPR = Rate over time. - both defined as Rates. (%) Figures are originated by the servicer of the debt pool. Each serviceer will have their own formats but will do info on prepayments, llosses, detauls on specific loans and so on.</skos:editorialNote>
		<skos:editorialNote xml:lang="en">The class Mortgage Pool originally had a property &apos;pool type&apos; referring to a selection list of textual stylings of pool types. Those are now replaced with actual sub types of mortgage pool. Here are the original notes and definition that went with the enumerated list of pool types: 

The type of pool for a pool backed security. Each of these pool types represents pools of mortgages that have conformed to certain standards (that change periodically) that make them &quot;conforming&quot; -- such as mortgage balance under a certain threshold, creditworthiness, loan-to-value, etc.

Further Notes:
Non Agency signifies a tranched security, for which there will also be a Tranche Type for the security tranche itself. All other pool types are Agency pool types. 

List Populated from Cutter document Page 5. 

Additional terms from Adept Advistory:
Under Agency mortgages, basically you have various types of pools under the various agencies. You have:
-GNMA-I
-GNMA-II
-GNMA Platinum
-FNMA 
-FHLMC
-FHLMC Gold
As far as definitions:The simple definition is that each of these pool types represents pools of mortgages that have conformed to certain standards (that change periodically) that make them &quot;conforming&quot; -- such as mortgage balance under a certain threshold, creditworthiness, loan-to-value, etc. Also, GNMA is explicitly backed by the US government, while FNMA and FHLMC are only implicitly backed by the US government. Perhaps there needs to be some research done on the parameters for what makes a loan conforming or not. 

Consensus:Review.</skos:editorialNote>
	</owl:Class>
	
	<owl:Class rdf:about="&fibo-sec-dbt-ab-mbs;MortgagePoolConstituent">
		<rdfs:subClassOf rdf:resource="&fibo-sec-dbt-ab-abs;LoanPoolConstituent"/>
		<rdfs:label xml:lang="en">mortgage pool constituent</rdfs:label>
		<skos:definition xml:lang="en">Amortgage defined as a constituent of a Mortgage Pool.</skos:definition>
	</owl:Class>
	
	<owl:Class rdf:about="&fibo-sec-dbt-ab-mbs;NonAgencyIOTranche">
		<rdfs:subClassOf rdf:resource="&fibo-sec-dbt-ab-mbs;TranchedMBSInstrument"/>
		<rdfs:label xml:lang="en">non agency i o tranche</rdfs:label>
		<skos:definition xml:lang="en">Interest Only tranche, meaning that this tranche will only pay interest.</skos:definition>
	</owl:Class>
	
	<owl:Class rdf:about="&fibo-sec-dbt-ab-mbs;NonAgencyJumpTranche">
		<rdfs:subClassOf rdf:resource="&fibo-sec-dbt-ab-mbs;TranchedMBSInstrument"/>
		<rdfs:subClassOf>
			<owl:Restriction>
				<owl:onProperty rdf:resource="&fibo-sec-dbt-ab-mbs;specifiesTrigger"/>
				<owl:someValuesFrom rdf:resource="&fibo-sec-dbt-ab-cmo;JumpZTriggerEvent"/>
			</owl:Restriction>
		</rdfs:subClassOf>
		<rdfs:label xml:lang="en">non agency jump tranche</rdfs:label>
		<skos:definition xml:lang="en">A tranche where if there is some sort of trigger event reached then the holders of the tranche will begin to receive payments.</skos:definition>
	</owl:Class>
	
	<owl:Class rdf:about="&fibo-sec-dbt-ab-mbs;NonAgencyJumpZTranche">
		<rdfs:subClassOf rdf:resource="&fibo-sec-dbt-ab-mbs;NonAgencyJumpTranche"/>
		<rdfs:subClassOf rdf:resource="&fibo-sec-dbt-ab-mbs;NonAgencyZTranche"/>
		<rdfs:label xml:lang="en">non agency jump z tranche</rdfs:label>
		<skos:definition xml:lang="en">A Jump Z tranche is like a Z tranche but if there is some sort of trigger event reached then the holders of the Jump Z tranche will begin to receive payments. Regular non-Sticky Jump Z tranches maintain their changed status only while the trigger event is in effect, and revert to their old payment status once the trigger event has passed.</skos:definition>
	</owl:Class>
	
	<owl:Class rdf:about="&fibo-sec-dbt-ab-mbs;NonAgencyMBSIssuer">
		<rdfs:subClassOf rdf:resource="&fibo-sec-dbt-ab-mbs;MBSIssuer"/>
		<rdfs:subClassOf>
			<owl:Class>
				<owl:unionOf rdf:parseType="Collection">
					<rdf:Description rdf:about="&fibo-fbc-fct-fse;Bank">
					</rdf:Description>
					<rdf:Description rdf:about="&fibo-sec-dbt-ab-mbs;SpecialistMortgageIssuer">
					</rdf:Description>
				</owl:unionOf>
			</owl:Class>
		</rdfs:subClassOf>
		<rdfs:label xml:lang="en">non agency m b s issuer</rdfs:label>
		<skos:definition xml:lang="en">A party which is a non agency issuer of MBS securities. The identity of this party may be a bank or a specialist (non agency) mortgage company. Term origin:MBS PoC Reviews</skos:definition>
	</owl:Class>
	
	<owl:Class rdf:about="&fibo-sec-dbt-ab-mbs;NonAgencyMortgagePool">
		<rdfs:subClassOf rdf:resource="&fibo-sec-dbt-ab-mbs;MortgagePool"/>
		<rdfs:label xml:lang="en">non agency mortgage pool</rdfs:label>
	</owl:Class>
	
	<owl:Class rdf:about="&fibo-sec-dbt-ab-mbs;NonAgencyPOTranche">
		<rdfs:subClassOf rdf:resource="&fibo-sec-dbt-ab-mbs;TranchedMBSInstrument"/>
		<rdfs:label xml:lang="en">non agency p o tranche</rdfs:label>
		<skos:definition xml:lang="en">Principal Only tranche. This tranche will only pay principal.</skos:definition>
	</owl:Class>
	
	<owl:Class rdf:about="&fibo-sec-dbt-ab-mbs;NonAgencyRegularJumpZTranche">
		<rdfs:subClassOf rdf:resource="&fibo-sec-dbt-ab-mbs;NonAgencyJumpZTranche"/>
		<rdfs:subClassOf>
			<owl:Restriction>
				<owl:onProperty rdf:resource="&fibo-sec-dbt-ab-mbs;reverts"/>
				<owl:someValuesFrom rdf:resource="&fibo-sec-dbt-ab-cmo;JumpZTriggerEventReversal"/>
			</owl:Restriction>
		</rdfs:subClassOf>
		<rdfs:label xml:lang="en">non agency regular jump z tranche</rdfs:label>
		<skos:definition xml:lang="en">Regular non-Sticky Jump Z tranches maintain their changed status only while the trigger event is in effect, and revert to their old payment status once the trigger event has passed.</skos:definition>
	</owl:Class>
	
	<owl:Class rdf:about="&fibo-sec-dbt-ab-mbs;NonAgencyStickyJumpZTranche">
		<rdfs:subClassOf rdf:resource="&fibo-sec-dbt-ab-mbs;NonAgencyJumpZTranche"/>
		<rdfs:label xml:lang="en">non agency sticky jump z tranche</rdfs:label>
		<skos:definition xml:lang="en">&quot;Sticky&quot; Jump Z tranches maintain the payment priority of a Jump Z tranche until they are retired.</skos:definition>
	</owl:Class>
	
	<owl:Class rdf:about="&fibo-sec-dbt-ab-mbs;NonAgencyZTranche">
		<rdfs:subClassOf rdf:resource="&fibo-sec-dbt-ab-mbs;TranchedMBSInstrument"/>
		<rdfs:label xml:lang="en">non agency z tranche</rdfs:label>
		<skos:definition xml:lang="en">A tranche that does not receive payments while other tranches remain.</skos:definition>
		<skos:editorialNote xml:lang="en">These tranches are credited for interest that would have been received and that interest is accrued to the Z tranche. Once all other tranches have been paid, the holders of the Z tranche receive payments. Types of Z Tranche: A Jump Z tranche is like a Z tranche but if there is some sort of trigger event reached then the holders of the Jump Z tranche will begin to receive payments. &quot;Sticky&quot; Jump Z tranches maintain this payment priority until they are retired, while regular, non-Sticky Jump Z tranches maintain their changed status only while the trigger event is in effect, and revert to their old payment status once the trigger event has passed. Review note: These are currently separate entries - they should be entries for types of Z Tranche. Add new list and move these to there.</skos:editorialNote>
	</owl:Class>
	
	<owl:Class rdf:about="&fibo-sec-dbt-ab-mbs;Pass-throughPool">
		<rdfs:subClassOf rdf:resource="&fibo-sec-dbt-ab-mbs;MortgagePool"/>
		<rdfs:label xml:lang="en">pass-through pool</rdfs:label>
		<skos:editorialNote xml:lang="en">REVIEW: These are all Pass-through so not clear why this term is here. Term originates with Cutter SME review but seems redundant. If not, this would be non mutually exclusive with agency pool. In general, agency MBS pools are pass through and non agency are tranched, but this reflects a business necessity not a logical necessity.</skos:editorialNote>
	</owl:Class>
	
	<owl:Class rdf:about="&fibo-sec-dbt-ab-mbs;PassThroughMBSDeal">
		<rdfs:subClassOf rdf:resource="&fibo-sec-dbt-ab-mbs;MBSDeal"/>
		<rdfs:subClassOf>
			<owl:Restriction>
				<owl:onProperty rdf:resource="&fibo-sec-dbt-ab-mbs;isAlso"/>
				<owl:someValuesFrom rdf:resource="&fibo-sec-dbt-ab-mbs;AgencyMBSDeal"/>
			</owl:Restriction>
		</rdfs:subClassOf>
		<rdfs:label xml:lang="en">pass through m b s deal</rdfs:label>
		<owl:disjointWith rdf:resource="&fibo-sec-dbt-ab-mbs;TranchedMBSDeal"/>
		<skos:definition xml:lang="en">An issue of Mortgage Backed Security instruments in which payments on the pool are passed through to investors</skos:definition>
		<skos:editorialNote xml:lang="en">The cashflows from interest and principal payments on the mortgages in the underlying pool are passed on to investors, usually with the deduction of fees in for them of a reduction in a mumber of percentage points or a monetary amount. Modeling note: Thinking about this further, and after more PoC reviews, it seems to me that we should simply define two kinds of Deal which are Tranched and Pass Thtrough, just below the level of Pool Backed Securities Deal. Investigaiton of various SMOs and REMICs and the like suggests that the original PoC term duality shown here (Tranched = Non Agency; Pass Through = Agency) is too simplistic.</skos:editorialNote>
	</owl:Class>
	
	<owl:Class rdf:about="&fibo-sec-dbt-ab-mbs;PassThroughMBSDealProspectus">
		<rdfs:subClassOf rdf:resource="&fibo-sec-dbt-ab-mbs;MBSDealProspectus"/>
		<rdfs:label xml:lang="en">pass through m b s deal prospectus</rdfs:label>
		<owl:disjointWith rdf:resource="&fibo-sec-dbt-ab-mbs;TranchedMBSDealProspectus"/>
		<skos:definition xml:lang="en">The written prospectus for an agency, pass through issue of Mortgage Backed Securities</skos:definition>
	</owl:Class>
	
	<owl:Class rdf:about="&fibo-sec-dbt-ab-mbs;PassThroughMBSInstrument">
		<rdfs:subClassOf rdf:resource="&fibo-sec-dbt-ab-mbs;MortgageBackedSecurityInstrument"/>
		<rdfs:subClassOf>
			<owl:Restriction>
				<owl:onProperty rdf:resource="&fibo-sec-dbt-ab-mbs;hasNote"/>
				<owl:someValuesFrom rdf:resource="&fibo-sec-dbt-ab-mbs;PassThroughMBSInstrumentNote"/>
			</owl:Restriction>
		</rdfs:subClassOf>
		<rdfs:label xml:lang="en">pass through m b s instrument</rdfs:label>
		<owl:disjointWith rdf:resource="&fibo-sec-dbt-ab-mbs;TranchedMBSInstrument"/>
		<skos:definition xml:lang="en">A security in which the cash flows from the underlying asset pool are passed through to the investor by way of redemption payments.</skos:definition>
	</owl:Class>
	
	<owl:Class rdf:about="&fibo-sec-dbt-ab-mbs;PassThroughMBSInstrumentNote">
		<rdfs:subClassOf rdf:resource="&fibo-sec-dbt-ab-mbs;SecurityNote"/>
		<rdfs:label xml:lang="en">pass through m b s instrument note</rdfs:label>
		<skos:definition xml:lang="en">An individual note of a pass through instrument.</skos:definition>
	</owl:Class>
	
	<owl:Class rdf:about="&fibo-sec-dbt-ab-mbs;PassThroughMBSIssueUnderwriter">
		<rdfs:subClassOf rdf:resource="&fibo-sec-sec-iss;SecurityUnderwriter"/>
		<rdfs:label xml:lang="en">pass through m b s issue underwriter</rdfs:label>
		<skos:definition xml:lang="en">The party which agrees to buy any certificates that are not bought by investors Term origin:MBS PoC Reviews</skos:definition>
	</owl:Class>
	
	<owl:Class rdf:about="&fibo-sec-dbt-ab-mbs;PayingAgent">
		<rdfs:subClassOf>
			<owl:Restriction>
				<owl:onProperty rdf:resource="&fibo-sec-dbt-ab-mbs;responsibleFor"/>
				<owl:someValuesFrom rdf:resource="&fibo-fnd-pas-psch;Payment"/>
			</owl:Restriction>
		</rdfs:subClassOf>
		<rdfs:label xml:lang="en">paying agent</rdfs:label>
	</owl:Class>
	
	<owl:Class rdf:about="&fibo-sec-dbt-ab-mbs;PrivateLabelMBSDeal">
		<rdfs:subClassOf rdf:resource="&fibo-sec-dbt-ab-mbs;MBSDeal"/>
		<rdfs:label xml:lang="en">private label m b s deal</rdfs:label>
	</owl:Class>
	
	<owl:Class rdf:about="&fibo-sec-dbt-ab-mbs;RegularFloaterTranche">
		<rdfs:subClassOf rdf:resource="&fibo-sec-dbt-ab-mbs;FloaterTranche"/>
		<rdfs:label xml:lang="en">regular floater tranche</rdfs:label>
		<owl:disjointWith rdf:resource="&fibo-sec-dbt-ab-mbs;SuperFloaterTranche"/>
		<skos:definition xml:lang="en">A floater tranche is a tranche that is keyed to an index and a spread. The spread is added to the index.</skos:definition>
		<fibo-fnd-utl-av:explanatoryNote xml:lang="en">For example, 3 month LIBOR +50 -- meaning that the coupon would be whatever the 3 month LIBOR is plus 50 basis points. This is not a continuously updated number, rather it resets at specified intervals.</fibo-fnd-utl-av:explanatoryNote>
	</owl:Class>
	
	<owl:Class rdf:about="&fibo-sec-dbt-ab-mbs;ResidentialMBS">
		<rdfs:subClassOf rdf:resource="&fibo-sec-dbt-ab-mbs;MortgageBackedSecurityInstrument"/>
		<rdfs:label xml:lang="en">residential m b s</rdfs:label>
		<skos:definition xml:lang="en">Residential Mortgage-Backed Securities, which are trust certificates (bonds) backed by a pool of residential mortgage loans.</skos:definition>
		<fibo-fnd-utl-av:explanatoryNote xml:lang="en">Notes from CESR: They are issued by banks and backed by an underlying pool of residential mortgages. There can be some distinctions between prime RMBS and sub-prime/non-conforming RMBS although there is no consensus about what constitutes a sub-prime/non-conforming mortgage in Europe.</fibo-fnd-utl-av:explanatoryNote>
	</owl:Class>
	
	<owl:Class rdf:about="&fibo-sec-dbt-ab-mbs;ResidualTranche">
		<rdfs:subClassOf rdf:resource="&fibo-sec-dbt-ab-mbs;TranchedMBSInstrument"/>
		<rdfs:label xml:lang="en">residual tranche</rdfs:label>
		<skos:definition xml:lang="en">Unknown Further notes: Verify whether Residual Tranche and Support Tranche are meant to be in the same list of types as PAC etc. i.e. can a tranche not be PAC and Residual? this looks suspicioulsy like two semantics.</skos:definition>
	</owl:Class>
	
	<owl:Class rdf:about="&fibo-sec-dbt-ab-mbs;SBA-Pool">
		<rdfs:subClassOf rdf:resource="&fibo-sec-dbt-ab-mbs;MortgagePool"/>
		<rdfs:label xml:lang="en">SBA pool</rdfs:label>
		<skos:editorialNote xml:lang="en">Unknown pool type, from Cutter SME reviews; other pool types listed under Agency are from or validated by AdeptAdvisory SME review.</skos:editorialNote>
	</owl:Class>
	
	<owl:Class rdf:about="&fibo-sec-dbt-ab-mbs;SecuritizedMortgagePool">
		<rdfs:label xml:lang="en">securitized mortgage pool</rdfs:label>
		<skos:definition xml:lang="en">A mortgage pool which is securitized as part of the issue of some mortgage backed security.</skos:definition>
		<fibo-fnd-utl-av:explanatoryNote xml:lang="en">This is a logical union of a non agency mortgage pool which is securitized and an agency mortgage pool which has been securitized.</fibo-fnd-utl-av:explanatoryNote>
	</owl:Class>
	
	<owl:Class rdf:about="&fibo-sec-dbt-ab-mbs;SecurityNote">
		<rdfs:label xml:lang="en">security note</rdfs:label>
		<skos:definition xml:lang="en">An individually denominated note within a security or tranche of a security, where this is issued in notes of different denominations.</skos:definition>
		<skos:editorialNote xml:lang="en">Introduced for MBS Proof of Concept, to model MBS tranches where one tranche may have notes of multiple denominations. Other applications of this concept are not known at present. Trivially, all securities could be said to be in &quot;notes&quot; in this sense but the term is not normally referred to.</skos:editorialNote>
	</owl:Class>
	
	<owl:Class rdf:about="&fibo-sec-dbt-ab-mbs;SeniorMBSTranche">
		<rdfs:subClassOf rdf:resource="&fibo-sec-dbt-ab-mbs;TranchedMBSInstrument"/>
		<rdfs:subClassOf>
			<owl:Restriction>
				<owl:onProperty rdf:resource="&fibo-sec-dbt-ab-mbs;seniorTo"/>
				<owl:someValuesFrom rdf:resource="&fibo-sec-dbt-ab-mbs;MezzanineMBSTranche"/>
			</owl:Restriction>
		</rdfs:subClassOf>
		<rdfs:label xml:lang="en">senior m b s tranche</rdfs:label>
		<skos:definition xml:lang="en">Specific kinds of tranche are modeled for example and investigation only and have been removed from the diagrams. These will be removed from the final model.</skos:definition>
	</owl:Class>
	
	<owl:Class rdf:about="&fibo-sec-dbt-ab-mbs;SpecialistMortgageIssuer">
		<rdfs:subClassOf rdf:resource="&fibo-be-fct-fct;FunctionalBusinessEntity"/>
		<rdfs:label xml:lang="en">specialist mortgage issuer</rdfs:label>
		<skos:definition xml:lang="en">A business organization that specialises in and exists for the issuance of mortgages to the general public.</skos:definition>
		<skos:editorialNote xml:lang="en">Possibly add: Building Society. these exist in the UK (though almost extinct) but have not come up in US-based reviews of the model. Also known as Friendly Societies. There may be analogous organisations in other parts of the world, e.g. South America??</skos:editorialNote>
	</owl:Class>
	
	<owl:Class rdf:about="&fibo-sec-dbt-ab-mbs;SubordinatedMBSTranche">
		<rdfs:subClassOf rdf:resource="&fibo-sec-dbt-ab-mbs;TranchedMBSInstrument"/>
		<rdfs:label xml:lang="en">subordinated m b s tranche</rdfs:label>
		<skos:definition xml:lang="en">Specific kinds of tranche are modeled for example and investigation only and have been removed from the diagrams. These will be removed from the final model.</skos:definition>
	</owl:Class>
	
	<owl:Class rdf:about="&fibo-sec-dbt-ab-mbs;SuperFloaterTranche">
		<rdfs:subClassOf rdf:resource="&fibo-sec-dbt-ab-mbs;FloaterTranche"/>
		<rdfs:label xml:lang="en">super floater tranche</rdfs:label>
	</owl:Class>
	
	<owl:Class rdf:about="&fibo-sec-dbt-ab-mbs;TrancheNonPayment">
		<rdfs:subClassOf rdf:resource="&fibo-loan-tem-ev;NonPayment"/>
		<rdfs:label xml:lang="en">tranche non payment</rdfs:label>
		<skos:definition xml:lang="en">Failure of a tranche of a tranched security to pay out. This may or may not be interpreted as a credit event.</skos:definition>
	</owl:Class>
	
	<owl:Class rdf:about="&fibo-sec-dbt-ab-mbs;TrancheRatingAtIssue">
		<rdfs:label xml:lang="en">tranche rating at issue</rdfs:label>
		<skos:definition xml:lang="en">The rating at issue of a tranche of a security. Note this is under review</skos:definition>
		<skos:editorialNote xml:lang="en">In the case of CDOs, senior and mezzanine tranches of a CDO issue are typically rated, with the former receiving ratings of A to AAA and the latter receiving ratings of B to BBB. The ratings reflect both the credit quality of underlying collateral as well as how much protection a given tranch is afforded by tranches that are subordinate to it. Review note: Remove this it&apos;s no different from an instrument.</skos:editorialNote>
	</owl:Class>
	
	<owl:Class rdf:about="&fibo-sec-dbt-ab-mbs;TrancheType">
		<rdfs:label xml:lang="en">tranche type</rdfs:label>
		<skos:definition xml:lang="en">the type of tranche in a tranched MBS security</skos:definition>
	</owl:Class>
	
	<owl:Class rdf:about="&fibo-sec-dbt-ab-mbs;TranchedMBSDeal">
		<rdfs:subClassOf rdf:resource="&fibo-sec-dbt-ab-mbs;MBSDeal"/>
		<rdfs:subClassOf>
			<owl:Restriction>
				<owl:onProperty rdf:resource="&fibo-sec-dbt-ab-mbs;isAlso.1"/>
				<owl:someValuesFrom rdf:resource="&fibo-sec-dbt-ab-mbs;PrivateLabelMBSDeal"/>
			</owl:Restriction>
		</rdfs:subClassOf>
		<rdfs:label xml:lang="en">tranched m b s deal</rdfs:label>
	</owl:Class>
	
	<owl:Class rdf:about="&fibo-sec-dbt-ab-mbs;TranchedMBSDealProspectus">
		<rdfs:subClassOf rdf:resource="&fibo-sec-dbt-ab-mbs;MBSDealProspectus"/>
		<rdfs:label xml:lang="en">tranched m b s deal prospectus</rdfs:label>
	</owl:Class>
	
	<owl:Class rdf:about="&fibo-sec-dbt-ab-mbs;TranchedMBSInstrument">
		<rdfs:subClassOf rdf:resource="&fibo-sec-dbt-ab-mbs;MortgageBackedSecurityInstrument"/>
		<rdfs:subClassOf>
			<owl:Restriction>
				<owl:onProperty rdf:resource="&fibo-sec-dbt-ab-mbs;cashflowPrecedence"/>
				<owl:allValuesFrom rdf:resource="&fibo-sec-dbt-ab-mbs;TranchedMBSInstrument"/>
			</owl:Restriction>
		</rdfs:subClassOf>
		<rdfs:subClassOf>
			<owl:Restriction>
				<owl:onProperty rdf:resource="&fibo-sec-dbt-ab-mbs;providesCreditSupportTo"/>
				<owl:allValuesFrom rdf:resource="&fibo-sec-dbt-ab-mbs;TranchedMBSInstrument"/>
			</owl:Restriction>
		</rdfs:subClassOf>
		<rdfs:subClassOf>
			<owl:Restriction>
				<owl:onProperty rdf:resource="&fibo-sec-dbt-ab-mbs;hasNote"/>
				<owl:someValuesFrom rdf:resource="&fibo-sec-dbt-ab-mbs;MBSTrancheNote"/>
			</owl:Restriction>
		</rdfs:subClassOf>
		<rdfs:subClassOf>
			<owl:Restriction>
				<owl:onProperty rdf:resource="&fibo-sec-dbt-ab-mbs;hasPotentialEvent"/>
				<owl:someValuesFrom rdf:resource="&fibo-sec-dbt-ab-mbs;TrancheNonPayment"/>
			</owl:Restriction>
		</rdfs:subClassOf>
		<rdfs:label xml:lang="en">tranched m b s instrument</rdfs:label>
	</owl:Class>
	
	<owl:Class rdf:about="&fibo-sec-dbt-ab-mbs;TranchedMBSIssueUnderwriter">
		<rdfs:subClassOf rdf:resource="&fibo-sec-sec-iss;SecurityUnderwriter"/>
		<rdfs:label xml:lang="en">tranched m b s issue underwriter</rdfs:label>
		<skos:definition xml:lang="en">The party which agrees to buy any certificates that are not bought by investors Term origin:MBS PoC Reviews</skos:definition>
	</owl:Class>
	
	<owl:Class rdf:about="&fibo-sec-dbt-ab-mbs;Trustee">
		<rdfs:subClassOf rdf:resource="&fibo-fnd-pty-pty;PartyInRole"/>
		<rdfs:label xml:lang="en">trustee</rdfs:label>
		<skos:definition xml:lang="en">A party which has some role in relation to some financial investment (portfolio, issue etc.) which is formally defined as being a &quot;Trustee&quot; in that context.</skos:definition>
		<skos:editorialNote xml:lang="en">Definition is a bit self referential at present. Working definition for this class (added April 2010 as making CDO Portfolio Trusttee a direct child of &quot;Party&quot; seemed too simplistic). Action: Other types of Trustee need to be added to this class.</skos:editorialNote>
	</owl:Class>
	
	<owl:ObjectProperty rdf:about="&fibo-sec-dbt-ab-mbs;cashflowPrecedence">
		<rdfs:label xml:lang="en">cashflow precedence</rdfs:label>
		<rdfs:domain rdf:resource="&fibo-sec-dbt-ab-mbs;TranchedMBSInstrument"/>
		<rdfs:range rdf:resource="&fibo-sec-dbt-ab-mbs;TranchedMBSInstrument"/>
		<owl:inverseOf rdf:resource="&fibo-sec-dbt-ab-mbs;providesCreditSupportTo"/>
	</owl:ObjectProperty>
	
	<owl:ObjectProperty rdf:about="&fibo-sec-dbt-ab-mbs;denomination">
		<rdfs:label xml:lang="en">denomination</rdfs:label>
		<rdfs:domain rdf:resource="&fibo-sec-dbt-ab-mbs;MBSTrancheNote"/>
		<rdfs:range rdf:resource="&fibo-fnd-acc-cur;MonetaryAmount"/>
		<skos:definition xml:lang="en">The currency amount in which the Note is denominated, for example $500 notes.</skos:definition>
	</owl:ObjectProperty>
	
	<owl:ObjectProperty rdf:about="&fibo-sec-dbt-ab-mbs;denomination.1">
		<rdfs:label xml:lang="en">denomination</rdfs:label>
		<rdfs:domain rdf:resource="&fibo-sec-dbt-ab-mbs;PassThroughMBSInstrumentNote"/>
		<rdfs:range rdf:resource="&fibo-fnd-acc-cur;MonetaryAmount"/>
		<skos:definition xml:lang="en">The currency amount in which the Note is denominated, for example $500 notes. This term added by symmettry with MBS Tranche Note. needs to be reviewed and validated.</skos:definition>
	</owl:ObjectProperty>
	
	<owl:ObjectProperty rdf:about="&fibo-sec-dbt-ab-mbs;hasNote">
		<rdfs:subPropertyOf rdf:resource="&fibo-fnd-rel-rel;hasPart"/>
		<rdfs:label xml:lang="en">has note</rdfs:label>
		<rdfs:domain rdf:resource="&fibo-sec-dbt-ab-mbs;MortgageBackedSecurityInstrument"/>
		<rdfs:range rdf:resource="&fibo-sec-dbt-ab-mbs;SecurityNote"/>
	</owl:ObjectProperty>
	
	<owl:ObjectProperty rdf:about="&fibo-sec-dbt-ab-mbs;hasPotentialEvent">
		<rdfs:label xml:lang="en">has potential event</rdfs:label>
		<rdfs:domain rdf:resource="&fibo-sec-dbt-ab-mbs;TranchedMBSInstrument"/>
		<rdfs:range rdf:resource="&fibo-sec-dbt-ab-mbs;TrancheNonPayment"/>
	</owl:ObjectProperty>
	
	<owl:ObjectProperty rdf:about="&fibo-sec-dbt-ab-mbs;isAlso">
		<rdfs:label xml:lang="en">is also</rdfs:label>
		<rdfs:domain rdf:resource="&fibo-sec-dbt-ab-mbs;PassThroughMBSDeal"/>
		<rdfs:range rdf:resource="&fibo-sec-dbt-ab-mbs;AgencyMBSDeal"/>
	</owl:ObjectProperty>
	
	<owl:ObjectProperty rdf:about="&fibo-sec-dbt-ab-mbs;isAlso.1">
		<rdfs:label xml:lang="en">is also</rdfs:label>
		<rdfs:domain rdf:resource="&fibo-sec-dbt-ab-mbs;TranchedMBSDeal"/>
		<rdfs:range rdf:resource="&fibo-sec-dbt-ab-mbs;PrivateLabelMBSDeal"/>
	</owl:ObjectProperty>
	
	<owl:ObjectProperty rdf:about="&fibo-sec-dbt-ab-mbs;isSliceOf">
		<rdfs:subPropertyOf rdf:resource="&fibo-fnd-rel-rel;isPartOf"/>
		<rdfs:label xml:lang="en">is slice of</rdfs:label>
		<rdfs:domain rdf:resource="&fibo-sec-dbt-ab-mbs;SecurityNote"/>
		<rdfs:range rdf:resource="&fibo-sec-dbt-ab-mbs;MortgageBackedSecurityInstrument"/>
		<owl:inverseOf rdf:resource="&fibo-sec-dbt-ab-mbs;hasNote"/>
	</owl:ObjectProperty>
	
	<owl:DatatypeProperty rdf:about="&fibo-sec-dbt-ab-mbs;passThrough">
		<rdfs:label xml:lang="en">pass through</rdfs:label>
		<rdfs:domain rdf:resource="&fibo-sec-dbt-ab-mbs;MBSDeal"/>
		<rdfs:domain rdf:resource="&fibo-sec-dbt-ab-mbs;MortgageBackedSecurityInstrument"/>
		<rdfs:range rdf:resource="&xsd;boolean"/>
		<skos:definition xml:lang="en">Whether the cash flows from the underlying asset pool are passed through to the investor by way of redemption payments.</skos:definition>
	</owl:DatatypeProperty>
	
	<owl:DatatypeProperty rdf:about="&fibo-sec-dbt-ab-mbs;passThrough.1">
		<rdfs:label xml:lang="en">pass through</rdfs:label>
		<rdfs:domain rdf:resource="&fibo-sec-dbt-ab-mbs;PassThroughMBSDeal"/>
		<rdfs:range rdf:resource="&xsd;boolean"/>
		<skos:definition xml:lang="en">Cash flows from the underlying asset pool are passed through to the investor by way of redemption payments.</skos:definition>
	</owl:DatatypeProperty>
	
	<owl:DatatypeProperty rdf:about="&fibo-sec-dbt-ab-mbs;passThrough.2">
		<rdfs:label xml:lang="en">pass through</rdfs:label>
		<rdfs:domain rdf:resource="&fibo-sec-dbt-ab-mbs;PassThroughMBSInstrument"/>
		<rdfs:range rdf:resource="&xsd;boolean"/>
		<skos:definition xml:lang="en">The cash flows from the underlying asset pool are passed through to the holder of this instrument by way of redemption payments.</skos:definition>
	</owl:DatatypeProperty>
	
	<owl:DatatypeProperty rdf:about="&fibo-sec-dbt-ab-mbs;passThrough.3">
		<rdfs:label xml:lang="en">pass through</rdfs:label>
		<rdfs:domain rdf:resource="&fibo-sec-dbt-ab-mbs;TranchedMBSDeal"/>
		<rdfs:range rdf:resource="&xsd;boolean"/>
		<skos:definition xml:lang="en">Cash flows from the underlying asset pool are not passed through to the investor by way of redemption payments. Instead a tranched structure is used.</skos:definition>
	</owl:DatatypeProperty>
	
	<owl:DatatypeProperty rdf:about="&fibo-sec-dbt-ab-mbs;passThrough.4">
		<rdfs:label xml:lang="en">pass through</rdfs:label>
		<rdfs:domain rdf:resource="&fibo-sec-dbt-ab-mbs;TranchedMBSInstrument"/>
		<rdfs:range rdf:resource="&xsd;boolean"/>
		<skos:definition xml:lang="en">The cash flows from the underlying asset pool are not passed directly through to the investor by way of redemption payments but are used to fund cashflows that are defined specifically for the tranche.</skos:definition>
	</owl:DatatypeProperty>
	
	<owl:DatatypeProperty rdf:about="&fibo-sec-dbt-ab-mbs;prime">
		<rdfs:label xml:lang="en">prime</rdfs:label>
		<rdfs:domain rdf:resource="&fibo-sec-dbt-ab-mbs;ResidentialMBS"/>
		<rdfs:range rdf:resource="&xsd;boolean"/>
		<skos:definition xml:lang="en">Whether the mortage pool is identified as Prime or not.</skos:definition>
	</owl:DatatypeProperty>
	
	<owl:ObjectProperty rdf:about="&fibo-sec-dbt-ab-mbs;providesCreditSupportTo">
		<rdfs:subPropertyOf rdf:resource="&fibo-sec-dbt-dbti;mayBeSubordinatedTo"/>
		<rdfs:label xml:lang="en">provides credit support to</rdfs:label>
		<rdfs:domain rdf:resource="&fibo-sec-dbt-ab-mbs;TranchedMBSInstrument"/>
		<rdfs:range rdf:resource="&fibo-sec-dbt-ab-mbs;TranchedMBSInstrument"/>
	</owl:ObjectProperty>
	
	<owl:ObjectProperty rdf:about="&fibo-sec-dbt-ab-mbs;responsibleFor">
		<rdfs:label xml:lang="en">responsible for</rdfs:label>
		<rdfs:domain rdf:resource="&fibo-sec-dbt-ab-mbs;PayingAgent"/>
		<rdfs:range rdf:resource="&fibo-fnd-pas-psch;Payment"/>
	</owl:ObjectProperty>
	
	<owl:ObjectProperty rdf:about="&fibo-sec-dbt-ab-mbs;reverts">
		<rdfs:label xml:lang="en">reverts</rdfs:label>
		<rdfs:domain rdf:resource="&fibo-sec-dbt-ab-mbs;NonAgencyRegularJumpZTranche"/>
		<rdfs:range rdf:resource="&fibo-sec-dbt-ab-cmo;JumpZTriggerEventReversal"/>
	</owl:ObjectProperty>
	
	<owl:ObjectProperty rdf:about="&fibo-sec-dbt-ab-mbs;seniorTo">
		<rdfs:subPropertyOf rdf:resource="&fibo-sec-dbt-ab-mbs;cashflowPrecedence"/>
		<rdfs:label xml:lang="en">senior to</rdfs:label>
		<rdfs:domain rdf:resource="&fibo-sec-dbt-ab-mbs;MezzanineMBSTranche"/>
		<rdfs:domain rdf:resource="&fibo-sec-dbt-ab-mbs;SeniorMBSTranche"/>
		<rdfs:range rdf:resource="&fibo-sec-dbt-ab-mbs;MezzanineMBSTranche"/>
		<rdfs:range rdf:resource="&fibo-sec-dbt-ab-mbs;SubordinatedMBSTranche"/>
		<skos:definition xml:lang="en">Specific kinds of tranche are modeled for example and investigation only and have been removed from the diagrams. These will be removed from the final model.</skos:definition>
	</owl:ObjectProperty>
	
	<owl:ObjectProperty rdf:about="&fibo-sec-dbt-ab-mbs;specifiesTrigger">
		<rdfs:label xml:lang="en">specifies trigger</rdfs:label>
		<rdfs:domain rdf:resource="&fibo-sec-dbt-ab-mbs;NonAgencyJumpTranche"/>
		<rdfs:range rdf:resource="&fibo-sec-dbt-ab-cmo;JumpZTriggerEvent"/>
		<skos:definition xml:lang="en">The event which, when it takes place, causes the Jump Z holders to begin receiving payments.</skos:definition>
	</owl:ObjectProperty>

</rdf:RDF>