<?xml version="1.0" encoding="UTF-8"?>
<!DOCTYPE rdf:RDF [
	<!ENTITY cmns-av "https://www.omg.org/spec/Commons/AnnotationVocabulary/">
	<!ENTITY dct "http://purl.org/dc/terms/">
	<!ENTITY fibo-der-drc-bsc "https://spec.edmcouncil.org/fibo/ontology/DER/DerivativesContracts/DerivativesBasics/">
	<!ENTITY fibo-der-drc-str "https://spec.edmcouncil.org/fibo/ontology/DER/DerivativesContracts/StructuredInstruments/">
	<!ENTITY fibo-fnd-utl-av "https://spec.edmcouncil.org/fibo/ontology/FND/Utilities/AnnotationVocabulary/">
	<!ENTITY fibo-sec-dbt-pbs "https://spec.edmcouncil.org/fibo/ontology/SEC/Debt/PoolBackedSecurities/">
	<!ENTITY owl "http://www.w3.org/2002/07/owl#">
	<!ENTITY rdf "http://www.w3.org/1999/02/22-rdf-syntax-ns#">
	<!ENTITY rdfs "http://www.w3.org/2000/01/rdf-schema#">
	<!ENTITY skos "http://www.w3.org/2004/02/skos/core#">
	<!ENTITY xsd "http://www.w3.org/2001/XMLSchema#">
]>
<rdf:RDF xml:base="https://spec.edmcouncil.org/fibo/ontology/DER/DerivativesContracts/StructuredInstruments/"
	xmlns:cmns-av="https://www.omg.org/spec/Commons/AnnotationVocabulary/"
	xmlns:dct="http://purl.org/dc/terms/"
	xmlns:fibo-der-drc-bsc="https://spec.edmcouncil.org/fibo/ontology/DER/DerivativesContracts/DerivativesBasics/"
	xmlns:fibo-der-drc-str="https://spec.edmcouncil.org/fibo/ontology/DER/DerivativesContracts/StructuredInstruments/"
	xmlns:fibo-fnd-utl-av="https://spec.edmcouncil.org/fibo/ontology/FND/Utilities/AnnotationVocabulary/"
	xmlns:fibo-sec-dbt-pbs="https://spec.edmcouncil.org/fibo/ontology/SEC/Debt/PoolBackedSecurities/"
	xmlns:owl="http://www.w3.org/2002/07/owl#"
	xmlns:rdf="http://www.w3.org/1999/02/22-rdf-syntax-ns#"
	xmlns:rdfs="http://www.w3.org/2000/01/rdf-schema#"
	xmlns:skos="http://www.w3.org/2004/02/skos/core#"
	xmlns:xsd="http://www.w3.org/2001/XMLSchema#">
	
	<owl:Ontology rdf:about="https://spec.edmcouncil.org/fibo/ontology/DER/DerivativesContracts/StructuredInstruments/">
		<rdfs:label xml:lang="en">Structured Instruments Ontology</rdfs:label>
		<dct:abstract>This ontology defines concepts common to pre-packaged structured finance investment strategies based on a host of underlying instruments, pools, or other assets.</dct:abstract>
		<dct:license rdf:datatype="&xsd;anyURI">http://opensource.org/licenses/MIT</dct:license>
		<owl:imports rdf:resource="https://spec.edmcouncil.org/fibo/ontology/DER/DerivativesContracts/DerivativesBasics/"/>
		<owl:imports rdf:resource="https://spec.edmcouncil.org/fibo/ontology/FND/Utilities/AnnotationVocabulary/"/>
		<owl:imports rdf:resource="https://spec.edmcouncil.org/fibo/ontology/SEC/Debt/PoolBackedSecurities/"/>
		<owl:imports rdf:resource="https://www.omg.org/spec/Commons/AnnotationVocabulary/"/>
		<owl:versionIRI rdf:resource="https://spec.edmcouncil.org/fibo/ontology/DER/DerivativesContracts/StructuredInstruments/"/>
		<fibo-fnd-utl-av:hasMaturityLevel rdf:resource="&fibo-fnd-utl-av;Provisional"/>
		<cmns-av:copyright>Copyright (c) 2023 EDM Council, Inc.</cmns-av:copyright>
	</owl:Ontology>
	
	<owl:Class rdf:about="&fibo-der-drc-str;BonusCertificate">
		<rdfs:subClassOf rdf:resource="&fibo-der-drc-str;ParticipationCertificate"/>
		<rdfs:label xml:lang="en">bonus certificate</rdfs:label>
		<skos:definition xml:lang="en">certificate that has minimum redemption is equal to the nominal value provided the barrier has not been breached, with a greater risk in relation to multiple underlying asset(s) (worst-of), allowing for a higher bonus level or lower barrier, and with a reduced risk compared to a direct investment into the underlying asset(s)</skos:definition>
		<skos:note xml:lang="en">if the barrier is breached the product becomes a tracker certificate.</skos:note>
		<cmns-av:adaptedFrom xml:lang="en">ISO 10962, Securities and related financial instruments - Classification of financial instruments (CFI) code, Fifth edition, 2021-06-15</cmns-av:adaptedFrom>
	</owl:Class>
	
	<owl:Class rdf:about="&fibo-der-drc-str;CapitalProtectedProduct">
		<rdfs:subClassOf rdf:resource="&fibo-der-drc-str;StructuredProduct"/>
		<rdfs:label xml:lang="en">capital-protected product</rdfs:label>
		<skos:definition xml:lang="en">structured product that participates in the performance of a financial asset, such as a stock, fund or index, while protecting the investor&apos;s capital</skos:definition>
		<cmns-av:explanatoryNote xml:lang="en">Depending on the product, they may participate to varying degrees in the underlying asset&apos;s upside and protect the capital either entirely or partially.</cmns-av:explanatoryNote>
	</owl:Class>
	
	<owl:Class rdf:about="&fibo-der-drc-str;LeveragedProduct">
		<rdfs:subClassOf rdf:resource="&fibo-der-drc-str;StructuredProduct"/>
		<rdfs:label xml:lang="en">leveraged product</rdfs:label>
		<skos:definition xml:lang="en">structured product that provides a further enhanced yield (over and above that of a yield-enhancement product), often without any limit to the upside participation, and frequently with a stop-loss in order to limit potential capital losses</skos:definition>
		<skos:example xml:lang="en">Leveraged certificates are examples of leveraged products; they provide enhanced participation to an underlying with inbuilt leverage. Leveraged exposure is also provided on the downside performance of the underlying. Another example is a call warrant, which is simply a call option that is traded in a securitized format. This format is interesting in order to be able to trade a call option on underlyings for which no exchange traded option market exists.</skos:example>
	</owl:Class>
	
	<owl:Class rdf:about="&fibo-der-drc-str;OutperformanceCertificate">
		<rdfs:subClassOf rdf:resource="&fibo-der-drc-str;ParticipationCertificate"/>
		<rdfs:label xml:lang="en">outperformance certificate</rdfs:label>
		<skos:definition xml:lang="en">certificate that allows disproportionate participation (outperformance) in positive performance above the strike, reflecting underlying price moves 1:1 (adjusted by the conversion ratio and any related fees), and whose risk is comparable to direct investment in the underlying asset(s)</skos:definition>
		<skos:example xml:lang="en">For example: You buy an outperformance certificate based on a stock. The certificate’s strike price is 100 Euros and its participation factor is 150 percent. If the price of the underlying stock surpasses the strike price of 100 Euros, you are rewarded with a 150 percent return, instead of just 100 percent. If the price of the stock climbs to 110 Euros, for example, the value of the certificate would be 115 Euros.</skos:example>
		<cmns-av:adaptedFrom xml:lang="en">ISO 10962, Securities and related financial instruments - Classification of financial instruments (CFI) code, Fifth edition, 2021-06-15</cmns-av:adaptedFrom>
	</owl:Class>
	
	<owl:Class rdf:about="&fibo-der-drc-str;ParticipationCertificate">
		<rdfs:subClassOf rdf:resource="&fibo-der-drc-str;ParticipationInstrument"/>
		<rdfs:subClassOf rdf:resource="&fibo-sec-dbt-pbs;StructuredFinanceInstrument"/>
		<rdfs:label xml:lang="en">participation certificate</rdfs:label>
		<skos:definition xml:lang="en">participation product that provides the possibility to participate in the gains or losses in the price of an asset, subject to counterparty risk</skos:definition>
		<cmns-av:explanatoryNote xml:lang="en">In many cases, certificates do not give the investor the right to receive dividend distributions from the underlying stocks or other assets. For example: You buy a bonus certificate issued by your bank which is based on a stock that pays annual dividends. During the certificate&apos;s term, the bank holds the underlying stock and receives the dividends. At the end of the term, the bank pays the predefined bonus, even though the actual price of the stock is lower (but not below the protection threshold).Depending on the type of certificate, the exact terms and conditions, and the contract&apos;s expiry date, it is possible that the investor may receive the underlying asset instead of money at the end of the investment term. That is often the case with discount certificates based on stocks, for example, when their price sits below the predetermined cap. If the certificate&apos;s issuer becomes insolvent, the assets which underly the certificate are considered part of the issuer&apos;s liquid assets. This is in contrast to owning actual securities or shares in investment funds, as these are segregated assets which remain the property of the investor if the broker or custodian bank fails.</cmns-av:explanatoryNote>
		<cmns-av:synonym xml:lang="en">bearer debt note</cmns-av:synonym>
		<cmns-av:synonym xml:lang="en">certificate</cmns-av:synonym>
	</owl:Class>
	
	<owl:Class rdf:about="&fibo-der-drc-str;ParticipationInstrument">
		<rdfs:subClassOf rdf:resource="&fibo-der-drc-str;StructuredProduct"/>
		<rdfs:label xml:lang="en">participation instrument</rdfs:label>
		<skos:definition xml:lang="en">structured product that provides the possibility to participate in the performance of an asset or basket of assets</skos:definition>
		<cmns-av:adaptedFrom xml:lang="en">ISO 10962, Securities and related financial instruments - Classification of financial instruments (CFI) code, Fifth edition, 2021-06-15</cmns-av:adaptedFrom>
		<cmns-av:explanatoryNote xml:lang="en">The construction is generally based on a low exercise price option (LEPO) (base value less discounted future dividends) which in some cases might be comparable to a direct investment in the underlying asset(s) or a LEPO combined with other options, which together provide the desired disbursement profile.</cmns-av:explanatoryNote>
		<cmns-av:explanatoryNote xml:lang="en">These assets could be anything, from equities, funds, bonds, ETFs indices to a mix of those. The most common participation products are tracker certificates, providing 1-to-1 participation to the performance of a basket of securities.</cmns-av:explanatoryNote>
		<cmns-av:synonym xml:lang="en">participation product</cmns-av:synonym>
	</owl:Class>
	
	<owl:Class rdf:about="&fibo-der-drc-str;StructuredProduct">
		<rdfs:subClassOf rdf:resource="&fibo-der-drc-bsc;DerivativeInstrument"/>
		<rdfs:label xml:lang="en">structured product</rdfs:label>
		<skos:definition xml:lang="en">security whose cash flow characteristics depend upon one or more indices or that have embedded forwards or options or securities where an investor&apos;s investment return and the issuer&apos;s payment obligations are contingent on, or highly sensitive to, changes in the value of underlying assets, indices, interest rates or cash flows</skos:definition>
		<cmns-av:adaptedFrom xml:lang="en">ISO 10962, Securities and related financial instruments - Classification of financial instruments (CFI) code, Fifth edition, 2021-06-15</cmns-av:adaptedFrom>
		<cmns-av:explanatoryNote xml:lang="en">A structured product is a pre-packaged structured finance investment strategy based on a single security, a basket of securities, options, indices, commodities, debt issuance or foreign currencies, and to a lesser extent, derivatives. Structured products are not homogeneous - there are numerous varieties of derivatives and underlying assets - but they can be classified under the aside categories. Typically, a desk will employ a specialized &apos;structurer&apos; to design and manage its structured-product offering.</cmns-av:explanatoryNote>
		<cmns-av:synonym xml:lang="en">market-linked investment</cmns-av:synonym>
		<cmns-av:synonym xml:lang="en">structured instrument</cmns-av:synonym>
	</owl:Class>
	
	<owl:Class rdf:about="&fibo-der-drc-str;TrackerCertificate">
		<rdfs:subClassOf rdf:resource="&fibo-der-drc-str;ParticipationCertificate"/>
		<rdfs:label xml:lang="en">tracker certificate</rdfs:label>
		<skos:definition xml:lang="en">certificate that reflects underlying price moves 1:1 (adjusted by conversion ratio and any related fees), in which the associated risk is comparable to direct investment in the underlying asset(s)</skos:definition>
		<skos:example xml:lang="en">Tracker certificates can be purchased on stock exchanges which they are listed on. Many of these certificates track underlying assets at a ratio of 1:100. That means that an investor can invest just a fraction of the amount which would be required to buy the actual underlying asset. For example: You invest in a tracker certificate which is based on a stock basket with a value of 10,000 Euros. Because the tracker certificate uses a ratio of 1:100, you only need to pay 100 Euros for the certificate. If the price of the underlying stocks goes up by 10 percent (to 11,000 Euros), the value of the certificate will also go up by 10 percent (to 110 Euros).</skos:example>
		<skos:example xml:lang="en">Trackers can be used to invest in the performance of multiple stocks, for example. A tracker certificate is a structured instrument that allows the investor to invest in an underlying asset without actually owning the asset. From an investor perspective, tracker certificates work much like investment funds. The tracker follows the price of an underlying asset (one or more stocks, for example). The investor buys a certificate based on the tracker. If the value of the underlying asset goes up, the value of the certificate goes up with it. If the underlying asset loses value, the certificate loses value.</skos:example>
		<cmns-av:adaptedFrom xml:lang="en">ISO 10962, Securities and related financial instruments - Classification of financial instruments (CFI) code, Fifth edition, 2021-06-15</cmns-av:adaptedFrom>
		<cmns-av:explanatoryNote xml:lang="en">Some tracker certificates have an expiry date. That means they only track an underlying asset for a predetermined length of time (one year, for example). The certificate matures at the end of that period, at which point you as the investor are paid out its going value at the time of expiry.</cmns-av:explanatoryNote>
		<cmns-av:explanatoryNote xml:lang="en">Tracker certificates can also be used to profit off negative price developments. This is the case with so-called bear tracker certificates which take a short position on the underlying asset.  Note that tracker certificates do not normally pay out dividends. If one holds a certificate which tracks the stock of a company which pay dividends, they will not receive them. However, they may receive some form of compensation from the certificate’s issuer in some cases.</cmns-av:explanatoryNote>
		<cmns-av:explanatoryNote xml:lang="en">Unlike investment funds – which are divided into shares and owned by investors – tracker certificates are simply debt claims against the issuer (the bank which offers them, for example). That means the underlying asset which you are investing in does not belong to you, but to the issuer. Shares of investment funds, on the other hand, are classified as segregated assets in some jurisdictions, such as Switzerland, and are owned by you as the shareholder rather than by the fund managers. In practice, investors are not likely to notice the difference. But whether you hold tracker certificates or fund shares makes a big difference when an investment company becomes insolvent. Tracker certificates are not protected against issuer bankruptcy, and fall into the pool of general debt claims against the bankrupt party. If the issuer of a tracker certificate goes bankrupt, you may very likely lose all or part of the money which you invested in the tracker certificate. This danger is known as counterparty risk. By investing in tracker certificates, you agree to carry the counterparty risk.</cmns-av:explanatoryNote>
	</owl:Class>
	
	<owl:Class rdf:about="&fibo-der-drc-str;YieldEnhancementProduct">
		<rdfs:subClassOf rdf:resource="&fibo-der-drc-str;StructuredProduct"/>
		<rdfs:label xml:lang="en">yield-enhancement product</rdfs:label>
		<skos:definition xml:lang="en">structured product that provides a predefined yield in return for a downside risk</skos:definition>
		<skos:example xml:lang="en">Well-known yield-enhancement products include reverse convertibles. They provide a predetermined yield per annum in return for the willingness of the investor to absorb downside risk of for example a stock, index, currency-pair or fund. Reverse convertibles come in a broad range of variations (with or without barrier, multiple underlyings and/or callability).</skos:example>
	</owl:Class>
	
	<owl:Class rdf:about="&fibo-sec-dbt-pbs;PrincipalProtectedNote">
		<rdfs:subClassOf rdf:resource="&fibo-der-drc-str;CapitalProtectedProduct"/>
	</owl:Class>
	
	<owl:Class rdf:about="&fibo-sec-dbt-pbs;StructuredFinanceInstrument">
		<rdfs:subClassOf rdf:resource="&fibo-der-drc-str;StructuredProduct"/>
	</owl:Class>

</rdf:RDF>