<?xml version="1.0" encoding="UTF-8"?>
<!DOCTYPE rdf:RDF [
	<!ENTITY dct "http://purl.org/dc/terms/">
	<!ENTITY fibo-fbc-fct-ra "https://spec.edmcouncil.org/fibo/ontology/FBC/FunctionalEntities/RegistrationAuthorities/">
	<!ENTITY fibo-fbc-fi-fi "https://spec.edmcouncil.org/fibo/ontology/FBC/FinancialInstruments/FinancialInstruments/">
	<!ENTITY fibo-fbc-fi-stl "https://spec.edmcouncil.org/fibo/ontology/FBC/FinancialInstruments/Settlement/">
	<!ENTITY fibo-fbc-pas-fpas "https://spec.edmcouncil.org/fibo/ontology/FBC/ProductsAndServices/FinancialProductsAndServices/">
	<!ENTITY fibo-fnd-acc-cur "https://spec.edmcouncil.org/fibo/ontology/FND/Accounting/CurrencyAmount/">
	<!ENTITY fibo-fnd-dt-bd "https://spec.edmcouncil.org/fibo/ontology/FND/DatesAndTimes/BusinessDates/">
	<!ENTITY fibo-fnd-dt-oc "https://spec.edmcouncil.org/fibo/ontology/FND/DatesAndTimes/Occurrences/">
	<!ENTITY fibo-fnd-gao-obj "https://spec.edmcouncil.org/fibo/ontology/FND/GoalsAndObjectives/Objectives/">
	<!ENTITY fibo-fnd-pas-pas "https://spec.edmcouncil.org/fibo/ontology/FND/ProductsAndServices/ProductsAndServices/">
	<!ENTITY fibo-fnd-qt-qtu "https://spec.edmcouncil.org/fibo/ontology/FND/Quantities/QuantitiesAndUnits/">
	<!ENTITY fibo-fnd-rel-rel "https://spec.edmcouncil.org/fibo/ontology/FND/Relations/Relations/">
	<!ENTITY fibo-fnd-utl-av "https://spec.edmcouncil.org/fibo/ontology/FND/Utilities/AnnotationVocabulary/">
	<!ENTITY owl "http://www.w3.org/2002/07/owl#">
	<!ENTITY rdf "http://www.w3.org/1999/02/22-rdf-syntax-ns#">
	<!ENTITY rdfs "http://www.w3.org/2000/01/rdf-schema#">
	<!ENTITY skos "http://www.w3.org/2004/02/skos/core#">
	<!ENTITY sm "http://www.omg.org/techprocess/ab/SpecificationMetadata/">
	<!ENTITY xsd "http://www.w3.org/2001/XMLSchema#">
]>
<rdf:RDF xml:base="https://spec.edmcouncil.org/fibo/ontology/FBC/FinancialInstruments/Settlement/"
	xmlns:dct="http://purl.org/dc/terms/"
	xmlns:fibo-fbc-fct-ra="https://spec.edmcouncil.org/fibo/ontology/FBC/FunctionalEntities/RegistrationAuthorities/"
	xmlns:fibo-fbc-fi-fi="https://spec.edmcouncil.org/fibo/ontology/FBC/FinancialInstruments/FinancialInstruments/"
	xmlns:fibo-fbc-fi-stl="https://spec.edmcouncil.org/fibo/ontology/FBC/FinancialInstruments/Settlement/"
	xmlns:fibo-fbc-pas-fpas="https://spec.edmcouncil.org/fibo/ontology/FBC/ProductsAndServices/FinancialProductsAndServices/"
	xmlns:fibo-fnd-acc-cur="https://spec.edmcouncil.org/fibo/ontology/FND/Accounting/CurrencyAmount/"
	xmlns:fibo-fnd-dt-bd="https://spec.edmcouncil.org/fibo/ontology/FND/DatesAndTimes/BusinessDates/"
	xmlns:fibo-fnd-dt-oc="https://spec.edmcouncil.org/fibo/ontology/FND/DatesAndTimes/Occurrences/"
	xmlns:fibo-fnd-gao-obj="https://spec.edmcouncil.org/fibo/ontology/FND/GoalsAndObjectives/Objectives/"
	xmlns:fibo-fnd-pas-pas="https://spec.edmcouncil.org/fibo/ontology/FND/ProductsAndServices/ProductsAndServices/"
	xmlns:fibo-fnd-qt-qtu="https://spec.edmcouncil.org/fibo/ontology/FND/Quantities/QuantitiesAndUnits/"
	xmlns:fibo-fnd-rel-rel="https://spec.edmcouncil.org/fibo/ontology/FND/Relations/Relations/"
	xmlns:fibo-fnd-utl-av="https://spec.edmcouncil.org/fibo/ontology/FND/Utilities/AnnotationVocabulary/"
	xmlns:owl="http://www.w3.org/2002/07/owl#"
	xmlns:rdf="http://www.w3.org/1999/02/22-rdf-syntax-ns#"
	xmlns:rdfs="http://www.w3.org/2000/01/rdf-schema#"
	xmlns:skos="http://www.w3.org/2004/02/skos/core#"
	xmlns:sm="http://www.omg.org/techprocess/ab/SpecificationMetadata/"
	xmlns:xsd="http://www.w3.org/2001/XMLSchema#">
	
	<owl:Ontology rdf:about="https://spec.edmcouncil.org/fibo/ontology/FBC/FinancialInstruments/Settlement/">
		<rdfs:label xml:lang="en">Settlement Ontology</rdfs:label>
		<dct:abstract>This ontology defines high-level concepts for settlement that are applicable across FIBO domain areas, such as for loans, securities, and derivatives.</dct:abstract>
		<dct:license rdf:datatype="&xsd;anyURI">http://opensource.org/licenses/MIT</dct:license>
		<sm:contentLanguage rdf:datatype="&xsd;anyURI">http://www.w3.org/standards/techs/owl#w3c_all</sm:contentLanguage>
		<sm:copyright>Copyright (c) 2018 EDM Council, Inc.</sm:copyright>
		<sm:dependsOn rdf:datatype="&xsd;anyURI">https://spec.edmcouncil.org/fibo/ontology/BE/</sm:dependsOn>
		<sm:dependsOn rdf:datatype="&xsd;anyURI">https://spec.edmcouncil.org/fibo/ontology/FBC/</sm:dependsOn>
		<sm:dependsOn rdf:datatype="&xsd;anyURI">https://spec.edmcouncil.org/fibo/ontology/FND/</sm:dependsOn>
		<sm:fileAbbreviation>fibo-fbc-fi-stl</sm:fileAbbreviation>
		<sm:filename>Settlement.rdf</sm:filename>
		<owl:imports rdf:resource="https://spec.edmcouncil.org/fibo/ontology/FBC/FinancialInstruments/FinancialInstruments/"/>
		<owl:imports rdf:resource="https://spec.edmcouncil.org/fibo/ontology/FBC/FunctionalEntities/RegistrationAuthorities/"/>
		<owl:imports rdf:resource="https://spec.edmcouncil.org/fibo/ontology/FBC/ProductsAndServices/FinancialProductsAndServices/"/>
		<owl:imports rdf:resource="https://spec.edmcouncil.org/fibo/ontology/FND/Accounting/CurrencyAmount/"/>
		<owl:imports rdf:resource="https://spec.edmcouncil.org/fibo/ontology/FND/DatesAndTimes/BusinessDates/"/>
		<owl:imports rdf:resource="https://spec.edmcouncil.org/fibo/ontology/FND/DatesAndTimes/Occurrences/"/>
		<owl:imports rdf:resource="https://spec.edmcouncil.org/fibo/ontology/FND/GoalsAndObjectives/Objectives/"/>
		<owl:imports rdf:resource="https://spec.edmcouncil.org/fibo/ontology/FND/ProductsAndServices/ProductsAndServices/"/>
		<owl:imports rdf:resource="https://spec.edmcouncil.org/fibo/ontology/FND/Quantities/QuantitiesAndUnits/"/>
		<owl:imports rdf:resource="https://spec.edmcouncil.org/fibo/ontology/FND/Relations/Relations/"/>
		<owl:imports rdf:resource="https://spec.edmcouncil.org/fibo/ontology/FND/Utilities/AnnotationVocabulary/"/>
		<owl:versionIRI rdf:resource="https://spec.edmcouncil.org/fibo/ontology/FBC/20180801/FinancialInstruments/Settlement/"/>
		<fibo-fnd-utl-av:hasMaturityLevel rdf:resource="&fibo-fnd-utl-av;Provisional"/>
	</owl:Ontology>
	
	<owl:NamedIndividual rdf:about="&fibo-fbc-fi-stl;CommodityDelivery">
		<rdf:type rdf:resource="&fibo-fbc-fi-stl;SecurityDeliveryMethod"/>
		<rdfs:label>commodity delivery</rdfs:label>
		<skos:definition>the transfer of some commodity as consideration in exchange for a security</skos:definition>
	</owl:NamedIndividual>
	
	<owl:NamedIndividual rdf:about="&fibo-fbc-fi-stl;CurrencyDelivery">
		<rdf:type rdf:resource="&fibo-fbc-fi-stl;SecurityDeliveryMethod"/>
		<rdfs:label>currency delivery</rdfs:label>
		<skos:definition>the transfer of currency as consideration in exchange for a security</skos:definition>
	</owl:NamedIndividual>
	
	<owl:NamedIndividual rdf:about="&fibo-fbc-fi-stl;DeliveryInCash">
		<rdf:type rdf:resource="&fibo-fbc-fi-stl;SecurityDeliveryMethod"/>
		<rdfs:label>delivery in cash</rdfs:label>
		<skos:definition>the transfer of cash as consideration in exchange for a security</skos:definition>
	</owl:NamedIndividual>
	
	<owl:NamedIndividual rdf:about="&fibo-fbc-fi-stl;DeliveryOfASecurity">
		<rdf:type rdf:resource="&fibo-fbc-fi-stl;SecurityDeliveryMethod"/>
		<rdfs:label>delivery of a security</rdfs:label>
		<skos:definition>the transfer of some other security as consideration in exchange for a security</skos:definition>
	</owl:NamedIndividual>
	
	<owl:NamedIndividual rdf:about="&fibo-fbc-fi-stl;DeliveryOfAnInstrument">
		<rdf:type rdf:resource="&fibo-fbc-fi-stl;SecurityDeliveryMethod"/>
		<rdfs:label>delivery of an instrument</rdfs:label>
		<skos:definition>the transfer of some other financial instrument as consideration in exchange for a security</skos:definition>
	</owl:NamedIndividual>
	
	<owl:Class rdf:about="&fibo-fbc-fi-stl;SecurityDeliveryMethod">
		<rdfs:subClassOf rdf:resource="&fibo-fnd-gao-obj;DistributionStrategy"/>
		<rdfs:label xml:lang="en">delivery method</rdfs:label>
		<skos:definition>the method specified for transferring a commodity, currency, security, cash or another instrument as defined in the settlement terms of the contract</skos:definition>
	</owl:Class>
	
	<owl:Class rdf:about="&fibo-fbc-fi-stl;Settlement">
		<rdfs:subClassOf rdf:resource="&fibo-fnd-dt-oc;OccurrenceKind"/>
		<rdfs:label xml:lang="en">settlement</rdfs:label>
		<skos:definition>the act of finalizing a transaction, concluding negotiations, finalizing accounting, exchanging consideration, and/or legally recording documents, as applicable, as a result of that transaction</skos:definition>
	</owl:Class>
	
	<owl:Class rdf:about="&fibo-fbc-fi-stl;SettlementConvention">
		<rdfs:subClassOf rdf:resource="&fibo-fnd-dt-bd;Convention"/>
		<rdfs:subClassOf>
			<owl:Restriction>
				<owl:onProperty rdf:resource="&fibo-fnd-qt-qtu;hasNumericValue"/>
				<owl:someValuesFrom rdf:resource="&xsd;decimal"/>
			</owl:Restriction>
		</rdfs:subClassOf>
		<rdfs:label>settlement convention</rdfs:label>
		<skos:definition>a convention employed to determine the closing date (from the stated settlement date) in the process of settling a transaction on which securities or interests in securities are delivered, usually against (in simultaneous exchange for) payment of some consideration</skos:definition>
		<fibo-fnd-utl-av:explanatoryNote>This is usually stated in the form &apos;T+n&apos; where n is the number of business days from the specified settlement date (T). There are no date roll rules,the T+n simply refers to the next available business days and is specified as a whole number.</fibo-fnd-utl-av:explanatoryNote>
	</owl:Class>
	
	<owl:DatatypeProperty rdf:about="&fibo-fbc-fi-stl;allowsContractualSettlement">
		<rdfs:label>allows contractual settlement</rdfs:label>
		<rdfs:domain rdf:resource="&fibo-fbc-pas-fpas;SettlementTerms"/>
		<rdfs:range rdf:resource="&xsd;boolean"/>
		<skos:definition>indicates whether the market allows contractual settlement</skos:definition>
	</owl:DatatypeProperty>
	
	<owl:ObjectProperty rdf:about="&fibo-fbc-fi-stl;hasPreferredSettlementCurrency">
		<rdfs:label>has preferred settlement currency</rdfs:label>
		<rdfs:domain rdf:resource="&fibo-fbc-pas-fpas;SettlementTerms"/>
		<rdfs:range rdf:resource="&fibo-fnd-acc-cur;Currency"/>
		<skos:definition>indicates the preferred currency for settlement purposes</skos:definition>
	</owl:ObjectProperty>
	
	<owl:DatatypeProperty rdf:about="&fibo-fbc-fi-stl;isFractionalEligible">
		<rdfs:label>is fractional eligible</rdfs:label>
		<rdfs:domain rdf:resource="&fibo-fbc-pas-fpas;SettlementTerms"/>
		<rdfs:range rdf:resource="&xsd;boolean"/>
		<skos:definition>indicates whether the security can contain fractional share/amounts</skos:definition>
	</owl:DatatypeProperty>
	
	<owl:DatatypeProperty rdf:about="&fibo-fbc-fi-stl;isFullyAutomatedSecuritiesTransferApplicable">
		<rdfs:label>is fully automated securities transfer applicable</rdfs:label>
		<rdfs:domain rdf:resource="&fibo-fbc-pas-fpas;SettlementTerms"/>
		<rdfs:range rdf:resource="&xsd;boolean"/>
		<skos:definition>indicates whether the security is to be held at the transfer agent as part of the FAST (Fully Automated Securities Transfer) program</skos:definition>
		<skos:editorialNote>Term is specific to DTCC / US context. Is there a more generic meaning similar to this which applies across different jurisdictions? If not this term should be defined with reference to this specific context.</skos:editorialNote>
		<fibo-fnd-utl-av:abbreviation>is FAST applicable</fibo-fnd-utl-av:abbreviation>
	</owl:DatatypeProperty>
	
	<owl:DatatypeProperty rdf:about="&fibo-fbc-fi-stl;isInterchangeable">
		<rdfs:label>is interchangeable</rdfs:label>
		<rdfs:domain rdf:resource="&fibo-fbc-pas-fpas;SettlementTerms"/>
		<rdfs:range rdf:resource="&xsd;boolean"/>
		<skos:definition>indicates whether or not the security is freely interchangeable with other securities of the same type</skos:definition>
	</owl:DatatypeProperty>
	
	<owl:Class rdf:about="&fibo-fbc-pas-fpas;SettlementTerms">
		<rdfs:subClassOf>
			<owl:Restriction>
				<owl:onProperty rdf:resource="&fibo-fbc-fct-ra;specifies"/>
				<owl:someValuesFrom rdf:resource="&fibo-fbc-fi-stl;SecurityDeliveryMethod"/>
			</owl:Restriction>
		</rdfs:subClassOf>
		<rdfs:subClassOf>
			<owl:Restriction>
				<owl:onProperty rdf:resource="&fibo-fbc-fct-ra;specifies"/>
				<owl:someValuesFrom rdf:resource="&fibo-fbc-fi-stl;SettlementConvention"/>
			</owl:Restriction>
		</rdfs:subClassOf>
		<rdfs:subClassOf>
			<owl:Restriction>
				<owl:onProperty rdf:resource="&fibo-fnd-rel-rel;appliesTo"/>
				<owl:someValuesFrom rdf:resource="&fibo-fbc-fi-stl;Settlement"/>
			</owl:Restriction>
		</rdfs:subClassOf>
	</owl:Class>

</rdf:RDF>