<?xml version="1.0" encoding="UTF-8"?>
<!DOCTYPE rdf:RDF [
	<!ENTITY dct "http://purl.org/dc/terms/">
	<!ENTITY fibo-fnd-aap-ppl "https://spec.edmcouncil.org/fibo/FND/AgentsAndPeople/People/">
	<!ENTITY fibo-fnd-dt-fd "https://spec.edmcouncil.org/fibo/FND/DatesAndTimes/FinancialDates/">
	<!ENTITY fibo-fnd-org-org "https://spec.edmcouncil.org/fibo/FND/Organizations/Organizations/">
	<!ENTITY fibo-fnd-pty-pty "https://spec.edmcouncil.org/fibo/FND/Parties/Parties/">
	<!ENTITY fibo-fnd-pty-rl "https://spec.edmcouncil.org/fibo/FND/Parties/Roles/">
	<!ENTITY fibo-fnd-rel-rel "https://spec.edmcouncil.org/fibo/FND/Relations/Relations/">
	<!ENTITY fibo-fnd-utl-av "https://spec.edmcouncil.org/fibo/FND/Utilities/AnnotationVocabulary/">
	<!ENTITY owl "http://www.w3.org/2002/07/owl#">
	<!ENTITY rdf "http://www.w3.org/1999/02/22-rdf-syntax-ns#">
	<!ENTITY rdfs "http://www.w3.org/2000/01/rdf-schema#">
	<!ENTITY skos "http://www.w3.org/2004/02/skos/core#">
	<!ENTITY sm "http://www.omg.org/techprocess/ab/SpecificationMetadata/">
	<!ENTITY xsd "http://www.w3.org/2001/XMLSchema#">
]>
<rdf:RDF
	xml:base="https://spec.edmcouncil.org/fibo/FND/Parties/Parties/"
	xmlns:dct="http://purl.org/dc/terms/"
	xmlns:fibo-fnd-aap-ppl="https://spec.edmcouncil.org/fibo/FND/AgentsAndPeople/People/"
	xmlns:fibo-fnd-dt-fd="https://spec.edmcouncil.org/fibo/FND/DatesAndTimes/FinancialDates/"
	xmlns:fibo-fnd-org-org="https://spec.edmcouncil.org/fibo/FND/Organizations/Organizations/"
	xmlns:fibo-fnd-pty-pty="https://spec.edmcouncil.org/fibo/FND/Parties/Parties/"
	xmlns:fibo-fnd-pty-rl="https://spec.edmcouncil.org/fibo/FND/Parties/Roles/"
	xmlns:fibo-fnd-rel-rel="https://spec.edmcouncil.org/fibo/FND/Relations/Relations/"
	xmlns:fibo-fnd-utl-av="https://spec.edmcouncil.org/fibo/FND/Utilities/AnnotationVocabulary/"
	xmlns:owl="http://www.w3.org/2002/07/owl#"
	xmlns:rdf="http://www.w3.org/1999/02/22-rdf-syntax-ns#"
	xmlns:rdfs="http://www.w3.org/2000/01/rdf-schema#"
	xmlns:skos="http://www.w3.org/2004/02/skos/core#"
	xmlns:sm="http://www.omg.org/techprocess/ab/SpecificationMetadata/"
	xmlns:xsd="http://www.w3.org/2001/XMLSchema#">
	
	<owl:Ontology
		rdf:about="https://spec.edmcouncil.org/fibo/FND/Parties/Parties/">
		<rdfs:label>Parties Ontology</rdfs:label>
		<dct:license
			rdf:datatype="&xsd;anyURI">http://www.omg.org/techprocess/ab/SpecificationMetadata/MITLicense</dct:license>
		<sm:contentLanguage
			rdf:datatype="&xsd;anyURI">http://www.omg.org/spec/ODM/</sm:contentLanguage>
		<sm:contentLanguage
			rdf:datatype="&xsd;anyURI">http://www.w3.org/standards/techs/owl#w3c_all</sm:contentLanguage>
		<sm:copyright>Copyright (c) 2013-2016 EDM Council, Inc.
Copyright (c) 2013-2016 Object Management Group, Inc.</sm:copyright>
		<sm:dependsOn
			rdf:datatype="&xsd;anyURI">https://spec.edmcouncil.org/fibo/FND/AgentsAndPeople/People/</sm:dependsOn>
		<sm:dependsOn
			rdf:datatype="&xsd;anyURI">https://spec.edmcouncil.org/fibo/FND/DatesAndTimes/FinancialDates/</sm:dependsOn>
		<sm:dependsOn
			rdf:datatype="&xsd;anyURI">https://spec.edmcouncil.org/fibo/FND/Organizations/Organizations/</sm:dependsOn>
		<sm:dependsOn
			rdf:datatype="&xsd;anyURI">https://spec.edmcouncil.org/fibo/FND/Parties/Roles/</sm:dependsOn>
		<sm:dependsOn
			rdf:datatype="&xsd;anyURI">https://spec.edmcouncil.org/fibo/FND/Relations/Relations/</sm:dependsOn>
		<sm:dependsOn
			rdf:datatype="&xsd;anyURI">https://spec.edmcouncil.org/fibo/FND/Utilities/AnnotationVocabulary/</sm:dependsOn>
		<sm:fileAbbreviation>fibo-fnd-pty-pty</sm:fileAbbreviation>
		<sm:fileAbstract>This ontology defines the high-level concepts of parties in roles, for use in other FIBO ontology elements. The concept of a party in a role describes some entity defined specifically in terms of some role which it performs in some formal contractual or transactional relationship. The ontology includes one or more basic party in role concepts. The ontology also includes one or more logical combinations of types of autonomous entity which may perform some of the party roles defined elsewhere in this ontology, such as the role of ownership.</sm:fileAbstract>
		<sm:filename>Parties.rdf</sm:filename>
		<rdfs:seeAlso
			rdf:datatype="&xsd;anyURI">https://spec.edmcouncil.org/fibo/AboutTheEDMC-FIBOFamily/</rdfs:seeAlso>
		<rdfs:seeAlso
			rdf:datatype="&xsd;anyURI">https://spec.edmcouncil.org/fibo/FND/AboutFND/</rdfs:seeAlso>
		<rdfs:seeAlso
			rdf:datatype="&xsd;anyURI">https://spec.edmcouncil.org/fibo/FND/Parties/AboutParties/</rdfs:seeAlso>
		<owl:imports
			rdf:resource="https://spec.edmcouncil.org/fibo/FND/AgentsAndPeople/People/"/>
		<owl:imports
			rdf:resource="https://spec.edmcouncil.org/fibo/FND/DatesAndTimes/FinancialDates/"/>
		<owl:imports
			rdf:resource="https://spec.edmcouncil.org/fibo/FND/Organizations/Organizations/"/>
		<owl:imports
			rdf:resource="https://spec.edmcouncil.org/fibo/FND/Parties/Roles/"/>
		<owl:imports
			rdf:resource="https://spec.edmcouncil.org/fibo/FND/Relations/Relations/"/>
		<owl:imports
			rdf:resource="https://spec.edmcouncil.org/fibo/FND/Utilities/AnnotationVocabulary/"/>
		<owl:versionIRI
			rdf:resource="https://spec.edmcouncil.org/fibo/FND/20160201/Parties/Parties/"/>
		<skos:changeNote>The http://www.omg.org/spec/FIBO/Foundations/20130601/Roles/Parties.owl version of the ontology was revised in advance of the September 2013 New Brunswick, NJ meeting, as follows:
   (1) to use slash style URI/IRIss (also called 303 URIs, vs. hash style) as required to support server side processing 
   (2) to use version-independent IRIs for all definitions internally as opposed to version-specific IRIs
   (3) to change the file suffix from .owl to .rdf to increase usability in RDF tools
   (4) to use 4-level abbreviations and corresponding namespace prefixes for all FIBO ontologies, reflecting a family/specification/module/ontology structure
   (5) to incorporate changes to the specification metadata to support documentation at the family, specification, module, and ontology level, similar to the abbreviations.
   (6) to combine Parties, Party Roles, and Roles in a single, new, Parties module, combine Parties and Party Roles into a single ontology, and add an inverse for the hasParty property.</skos:changeNote>
		<skos:changeNote>The https://spec.edmcouncil.org/fibo/FND/20130801/Parties/Parties.rdf version of the ontology was was modified per the issue resolutions identified in the FIBO FND 1.0 FTF report and in http://spec.edmcouncil.org/fibo/FND/1.0/AboutFND-1.0/.</skos:changeNote>
		<skos:changeNote>The https://spec.edmcouncil.org/fibo/FND/20141101/Parties/Parties.rdf version of this ontology was revised as a part of the issue resolutions identified in the FIBO FND 1.1 RTF report to add a parent of hasDate to date properties.</skos:changeNote>
	</owl:Ontology>
	
	<owl:Class
		rdf:about="&fibo-fnd-pty-pty;IndependentParty">
		<rdfs:subClassOf>
			<owl:Class>
				<owl:unionOf>
					<rdf:Description>
						<rdf:first
							rdf:resource="&fibo-fnd-aap-ppl;Person"/>
						<rdf:rest>
							<rdf:Description>
								<rdf:first
									rdf:resource="&fibo-fnd-org-org;Organization"/>
								<rdf:rest
									rdf:resource="&rdf;nil"/>
							</rdf:Description>
						</rdf:rest>
					</rdf:Description>
				</owl:unionOf>
			</owl:Class>
		</rdfs:subClassOf>
		<rdfs:label>independent party</rdfs:label>
		<skos:definition>any person or organization capable of performing any business party role, such as an individual, a corporation, a partnership, an association, a joint-stock company, a business trust, or an unincorporated organization</skos:definition>
		<fibo-fnd-utl-av:adaptedFrom
			rdf:datatype="&xsd;anyURI">www.ecfr.gov</fibo-fnd-utl-av:adaptedFrom>
	</owl:Class>
	
	<owl:Class
		rdf:about="&fibo-fnd-pty-pty;OrganizationMember">
		<rdfs:subClassOf
			rdf:resource="&fibo-fnd-pty-pty;PartyInRole"/>
		<rdfs:subClassOf>
			<owl:Restriction>
				<owl:onProperty
					rdf:resource="&fibo-fnd-pty-rl;isPlayedBy"/>
				<owl:someValuesFrom>
					<owl:Restriction>
						<owl:allValuesFrom
							rdf:resource="&fibo-fnd-org-org;Organization"/>
						<owl:onProperty
							rdf:resource="&fibo-fnd-rel-rel;isMemberOf"/>
					</owl:Restriction>
				</owl:someValuesFrom>
			</owl:Restriction>
		</rdfs:subClassOf>
		<rdfs:label>organization member</rdfs:label>
		<skos:definition>identifies that which has a membership role in some organization</skos:definition>
	</owl:Class>
	
	<owl:Class
		rdf:about="&fibo-fnd-pty-pty;PartyInRole">
		<rdfs:subClassOf
			rdf:resource="&fibo-fnd-pty-rl;AgentInRole"/>
		<rdfs:subClassOf>
			<owl:Restriction>
				<owl:onClass
					rdf:resource="&fibo-fnd-dt-fd;Date"/>
				<owl:onProperty
					rdf:resource="&fibo-fnd-pty-pty;hasCommencementDate"/>
				<owl:qualifiedCardinality
					rdf:datatype="&xsd;nonNegativeInteger">1</owl:qualifiedCardinality>
			</owl:Restriction>
		</rdfs:subClassOf>
		<rdfs:subClassOf>
			<owl:Restriction>
				<owl:onClass
					rdf:resource="&fibo-fnd-pty-pty;IndependentParty"/>
				<owl:onProperty
					rdf:resource="&fibo-fnd-rel-rel;hasIdentity"/>
				<owl:qualifiedCardinality
					rdf:datatype="&xsd;nonNegativeInteger">1</owl:qualifiedCardinality>
			</owl:Restriction>
		</rdfs:subClassOf>
		<rdfs:label>party in role</rdfs:label>
		<skos:definition>a relative concept that ties an independent party to a specific role they are standing in in which they play some part i.e. are party to</skos:definition>
		<skos:example>Examples include organization member, issuer, owner, partner in a partnership, shareholder, etc.</skos:example>
		<skos:scopeNote>The concept of a party in a role refers only to those contexts in which in natural English one would call someone a &apos;party&apos; for example being party to a contract or to a transaction; it does not cover entities as performing some role in some activity or process (the separate concept Actor covers that). A good test is whether the relative thing defined as PartyInRole can be sensibly said to have a part or play a part in something. Corresponds to the English (not data modeling) sense of the word &apos;Party&apos;.</skos:scopeNote>
		<fibo-fnd-utl-av:adaptedFrom>OMG Property and Casualty Information Models, dtc/12-01-04, Annex A, Glossary of Data Model Terms and Definitions</fibo-fnd-utl-av:adaptedFrom>
	</owl:Class>
	
	<owl:ObjectProperty
		rdf:about="&fibo-fnd-pty-pty;hasCommencementDate">
		<rdfs:subPropertyOf
			rdf:resource="&fibo-fnd-dt-fd;hasStartDate"/>
		<rdfs:label>has commencement date</rdfs:label>
		<rdfs:domain
			rdf:resource="&fibo-fnd-pty-pty;PartyInRole"/>
		<rdfs:range
			rdf:resource="&fibo-fnd-dt-fd;Date"/>
		<skos:definition>the date a party relationship comes into force</skos:definition>
	</owl:ObjectProperty>
	
	<owl:ObjectProperty
		rdf:about="&fibo-fnd-pty-pty;hasParty">
		<rdfs:subPropertyOf
			rdf:resource="&fibo-fnd-rel-rel;has"/>
		<rdfs:label>has party</rdfs:label>
		<rdfs:range
			rdf:resource="&fibo-fnd-pty-pty;IndependentParty"/>
		<skos:definition>identifies an independent party associated with an agreement, contract, policy, regulation, or other business arrangement</skos:definition>
	</owl:ObjectProperty>
	
	<owl:ObjectProperty
		rdf:about="&fibo-fnd-pty-pty;hasPartyIdentity">
		<rdfs:label>has party identity</rdfs:label>
	</owl:ObjectProperty>
	
	<owl:ObjectProperty
		rdf:about="&fibo-fnd-pty-pty;hasPartyInRole">
		<rdfs:subPropertyOf
			rdf:resource="&fibo-fnd-rel-rel;has"/>
		<rdfs:label>has party in role</rdfs:label>
		<rdfs:range
			rdf:resource="&fibo-fnd-pty-pty;PartyInRole"/>
		<skos:definition>identifies a party acting in a specific role as related to the particular agreement, contract, policy, regulation, or other business relationship</skos:definition>
	</owl:ObjectProperty>
	
	<owl:ObjectProperty
		rdf:about="&fibo-fnd-pty-pty;isAPartyTo">
		<rdfs:label>is a party to</rdfs:label>
		<rdfs:domain
			rdf:resource="&fibo-fnd-pty-pty;IndependentParty"/>
		<owl:inverseOf
			rdf:resource="&fibo-fnd-pty-pty;hasParty"/>
		<skos:definition>identifies an agreement, contract, policy, regulation, or other business transaction that an independent party is associated with</skos:definition>
		<fibo-fnd-utl-av:explanatoryNote>This property should be read referring to some context (known as a &apos;mediating thing&apos; in the informative upper ontology).</fibo-fnd-utl-av:explanatoryNote>
	</owl:ObjectProperty>
	
	<owl:ObjectProperty
		rdf:about="&fibo-fnd-pty-pty;isPartyInRelationTo">
		<rdfs:label>is party in relation to</rdfs:label>
	</owl:ObjectProperty>

</rdf:RDF>