<?xml version="1.0" encoding="UTF-8"?>
<!DOCTYPE rdf:RDF [
	<!ENTITY fibo-be-le-fbo "https://spec.edmcouncil.org/fibo/BE/LegalEntities/FormalBusinessOrganizations/">
	<!ENTITY fibo-be-oac-cpty "https://spec.edmcouncil.org/fibo/BE/OwnershipAndControl/ControlParties/">
	<!ENTITY fibo-be-oacx-cpx "https://spec.edmcouncil.org/fibo/BE/OwnershipAndControlExt/ControlPartiesExtras/">
	<!ENTITY fibo-fnd-agr-ctr "https://spec.edmcouncil.org/fibo/FND/Agreements/Contracts/">
	<!ENTITY fibo-fnd-pty-pty "https://spec.edmcouncil.org/fibo/FND/Parties/Parties/">
	<!ENTITY fibo-fnd-rel-rel "https://spec.edmcouncil.org/fibo/FND/Relations/Relations/">
	<!ENTITY fibo-fnd-utl-av "https://spec.edmcouncil.org/fibo/FND/Utilities/AnnotationVocabulary/">
	<!ENTITY owl "http://www.w3.org/2002/07/owl#">
	<!ENTITY rdf "http://www.w3.org/1999/02/22-rdf-syntax-ns#">
	<!ENTITY rdfs "http://www.w3.org/2000/01/rdf-schema#">
	<!ENTITY skos "http://www.w3.org/2004/02/skos/core#">
	<!ENTITY terms "http://purl.org/dc/terms/">
	<!ENTITY xsd "http://www.w3.org/2001/XMLSchema#">
]>
<rdf:RDF xml:base="https://spec.edmcouncil.org/fibo/BE/OwnershipAndControlExt/ControlPartiesExtras/"
	xmlns:fibo-be-le-fbo="https://spec.edmcouncil.org/fibo/BE/LegalEntities/FormalBusinessOrganizations/"
	xmlns:fibo-be-oac-cpty="https://spec.edmcouncil.org/fibo/BE/OwnershipAndControl/ControlParties/"
	xmlns:fibo-be-oacx-cpx="https://spec.edmcouncil.org/fibo/BE/OwnershipAndControlExt/ControlPartiesExtras/"
	xmlns:fibo-fnd-agr-ctr="https://spec.edmcouncil.org/fibo/FND/Agreements/Contracts/"
	xmlns:fibo-fnd-pty-pty="https://spec.edmcouncil.org/fibo/FND/Parties/Parties/"
	xmlns:fibo-fnd-rel-rel="https://spec.edmcouncil.org/fibo/FND/Relations/Relations/"
	xmlns:fibo-fnd-utl-av="https://spec.edmcouncil.org/fibo/FND/Utilities/AnnotationVocabulary/"
	xmlns:owl="http://www.w3.org/2002/07/owl#"
	xmlns:rdf="http://www.w3.org/1999/02/22-rdf-syntax-ns#"
	xmlns:rdfs="http://www.w3.org/2000/01/rdf-schema#"
	xmlns:skos="http://www.w3.org/2004/02/skos/core#"
	xmlns:terms="http://purl.org/dc/terms/"
	xmlns:xsd="http://www.w3.org/2001/XMLSchema#">
	
	<owl:Ontology rdf:about="https://spec.edmcouncil.org/fibo/BE/OwnershipAndControlExt/ControlPartiesExtras/">
		<rdfs:label xml:lang="en">ControlPartiesExtras</rdfs:label>
		<owl:imports rdf:resource="http://www.w3.org/2004/02/skos/core"/>
		<owl:imports rdf:resource="https://spec.edmcouncil.org/fibo/BE/LegalEntities/FormalBusinessOrganizations/"/>
		<owl:imports rdf:resource="https://spec.edmcouncil.org/fibo/BE/OwnershipAndControl/ControlParties/"/>
		<owl:imports rdf:resource="https://spec.edmcouncil.org/fibo/FND/Agreements/Contracts/"/>
		<owl:imports rdf:resource="https://spec.edmcouncil.org/fibo/FND/Parties/Parties/"/>
		<owl:imports rdf:resource="https://spec.edmcouncil.org/fibo/FND/Relations/Relations/"/>
		<owl:imports rdf:resource="https://spec.edmcouncil.org/fibo/FND/Utilities/AnnotationVocabulary/"/>
		<owl:versionIRI rdf:resource="https://spec.edmcouncil.org/fibo/BE/OwnershipAndControlExt/ControlPartiesExtras/"/>
		<fibo-fnd-utl-av:hasMaturityLevel rdf:resource="&fibo-fnd-utl-av;Informative"/>
	</owl:Ontology>
	
	<owl:Class rdf:about="&fibo-be-oac-cpty;ContractualControl">
		<rdfs:subClassOf>
			<owl:Restriction>
				<owl:onProperty rdf:resource="&fibo-be-oacx-cpx;contractualDeJureControlConferredBy"/>
				<owl:someValuesFrom rdf:resource="&fibo-be-oacx-cpx;ControlRelatedContract"/>
			</owl:Restriction>
		</rdfs:subClassOf>
	</owl:Class>
	
	<owl:Class rdf:about="&fibo-be-oac-cpty;LimitedDeFactoControl">
		<terms:description xml:lang="en">The ability to direct the affairs of some entity within prescribed limits. Those limits are described in terms of activities which the entity holding such control may cause the controlled entity to carry out.</terms:description>
	</owl:Class>
	
	<owl:Class rdf:about="&fibo-be-oacx-cpx;ControlRelatedContract">
		<rdfs:subClassOf rdf:resource="&fibo-fnd-agr-ctr;Contract"/>
		<rdfs:label xml:lang="en">control related contract</rdfs:label>
		<skos:definition xml:lang="en">A contract in which one party agrees to confer some degree and type of control upon the other party to that contract.</skos:definition>
	</owl:Class>
	
	<owl:ObjectProperty rdf:about="&fibo-be-oacx-cpx;contractualDeJureControlConferredBy">
		<rdfs:subPropertyOf rdf:resource="&fibo-fnd-rel-rel;isConferredBy"/>
		<rdfs:label xml:lang="en">contractual de jure control conferred by</rdfs:label>
		<rdfs:domain rdf:resource="&fibo-be-oac-cpty;ContractualControl"/>
		<rdfs:range rdf:resource="&fibo-be-oacx-cpx;ControlRelatedContract"/>
		<skos:definition xml:lang="en">Contractual Control is conferred by some contract in which one party agrees to confer some degree and type of control upon the other party to that contract.</skos:definition>
	</owl:ObjectProperty>
	
	<owl:ObjectProperty rdf:about="&fibo-be-oacx-cpx;controlIsInRespectTo">
		<rdfs:label xml:lang="en">control is in respect to</rdfs:label>
		<rdfs:domain rdf:resource="&fibo-be-oac-cpty;LimitedDeFactoControl"/>
		<skos:scopeNote xml:lang="en">Defines a kind of control which may be described in percentage terms or otherwise, as being control other than absolute, and therefore needing to be defined in terms of what are the activities on the part of the controlled entity, which the entity holding this control is able to direct the entity to do or not do. Scope Note: This is the basic relationship to &quot;any&quot; kind of activity; to define specific kinds of control one needs to define specific kinds of activity such as the ability to hire or replace executives, the ability to alter the capital structure of the entity, and so on. Types of control defined in terms of activities which regulators or (via statute), sovereigns may compel or prevent an entity doing, would also be framed in terms of extensions to the &quot;Activity&quot; and refinements of this relationship (either as sub-properties of or as restrictions on this relationship).</skos:scopeNote>
	</owl:ObjectProperty>
	
	<owl:ObjectProperty rdf:about="&fibo-be-oacx-cpx;deJureControllingInterestPartyHasIdentity">
		<rdfs:subPropertyOf rdf:resource="&fibo-fnd-rel-rel;hasIdentity"/>
		<rdfs:label xml:lang="en">de jure controlling interest party has identity</rdfs:label>
		<rdfs:range rdf:resource="&fibo-fnd-pty-pty;IndependentParty"/>
		<skos:definition xml:lang="en">That which performs the role of De Jure Controlling Party.</skos:definition>
		<fibo-fnd-utl-av:explanatoryNote xml:lang="en">This may be any form of potential owning party, that is a person, legal person, legitimate organization or formal organization (anything which is able to hold and own formal ownership instruments of some sort).</fibo-fnd-utl-av:explanatoryNote>
	</owl:ObjectProperty>
	
	<owl:ObjectProperty rdf:about="&fibo-be-oacx-cpx;effectivelyExercises">
		<rdfs:label xml:lang="en">effectively exercises</rdfs:label>
		<rdfs:range rdf:resource="&fibo-be-oac-cpty;InvestmentBasedDeFactoControl"/>
		<skos:definition xml:lang="en">The Investment Owning Party effectively exercises some degree of de facto control as a result of their interest in the entity.</skos:definition>
	</owl:ObjectProperty>
	
	<owl:ObjectProperty rdf:about="&fibo-be-oacx-cpx;entityControllingPartyIdentity">
		<rdfs:subPropertyOf rdf:resource="&fibo-fnd-rel-rel;hasIdentity"/>
		<rdfs:label xml:lang="en">entity controlling party identity</rdfs:label>
		<rdfs:range rdf:resource="&fibo-fnd-pty-pty;IndependentParty"/>
		<skos:definition xml:lang="en">That which is able to be the Entity Controlling Party. Scope Note: It is assumed that since control follows from some form of ownership or contractual instrument, that the range of entities which may fulfil this party role is the same as that for entity ownership, namely &quot;Involved Party&quot;; that is, a logical union of natural persons, legal persons and formal organizations.</skos:definition>
	</owl:ObjectProperty>
	
	<owl:ObjectProperty rdf:about="&fibo-be-oacx-cpx;exercisesMajorityOf">
		<rdfs:label xml:lang="en">exercises majority of</rdfs:label>
		<rdfs:range rdf:resource="&fibo-be-oac-cpty;DegreeOfControl"/>
		<skos:definition xml:lang="en">Exercises, either alone or in equal degree with other such parties, majority De Facto Control over the entity in respect of which this party is defined.</skos:definition>
	</owl:ObjectProperty>
	
	<owl:ObjectProperty rdf:about="&fibo-be-oacx-cpx;exercisesSomeDegreeOfControlOver">
		<rdfs:label xml:lang="en">exercises some degree of control over</rdfs:label>
		<rdfs:range rdf:resource="&fibo-be-le-fbo;FormallyConstitutedOrganization"/>
	</owl:ObjectProperty>
	
	<owl:ObjectProperty rdf:about="&fibo-be-oacx-cpx;generalPartnerExercises">
		<rdfs:label xml:lang="en">general partner exercises</rdfs:label>
		<rdfs:range rdf:resource="&fibo-be-oac-cpty;ConstitutionalDeJureControl"/>
		<skos:definition xml:lang="en">The General Partner exercises control as a result of holding General Partner equity, which is therefore a form of constitutional control of the entity.</skos:definition>
	</owl:ObjectProperty>
	
	<owl:ObjectProperty rdf:about="&fibo-be-oacx-cpx;hasDeFactoControllingInterestParty">
		<rdfs:label xml:lang="en">has de facto controlling interest party</rdfs:label>
		<rdfs:range rdf:resource="&fibo-be-oac-cpty;DeFactoControllingInterestParty"/>
		<skos:definition xml:lang="en">Some party which exercises some de facto control over the Formal Organization.</skos:definition>
	</owl:ObjectProperty>
	
	<owl:ObjectProperty rdf:about="&fibo-be-oacx-cpx;hasDeJureControllingInterestParty">
		<rdfs:label xml:lang="en">has de jure controlling interest party</rdfs:label>
		<rdfs:range rdf:resource="&fibo-be-oac-cpty;DeJureControllingInterestParty"/>
		<skos:definition xml:lang="en">The Formal Organization is legally controlled in some way by some de jure controlling party, that is some entity which exercises legally based control.</skos:definition>
	</owl:ObjectProperty>

</rdf:RDF>