<?xml version="1.0" encoding="UTF-8"?>
  
<!DOCTYPE rdf:RDF [
    <!ENTITY fibo-be-oacx-cptyx "http://spec.edmcouncil.org/fibo/red/be/ownership-control-ext/control-parties-extras/">
    <!ENTITY fibo-fnd-agr-ctr "http://spec.edmcouncil.org/fibo/red/fnd/agreements/contracts/">
    <!ENTITY fibo-fnd-pty-pty "http://spec.edmcouncil.org/fibo/red/fnd/parties/parties/">
    <!ENTITY fibo-be-le-fbo "http://spec.edmcouncil.org/fibo/red/be/legal-entities/formal-business-organizations/">
    <!ENTITY fibo-fnd-law-lcap "http://spec.edmcouncil.org/fibo/red/fnd/law/legal-capacities/">
    <!ENTITY fibo-be-ptr-ptr "http://spec.edmcouncil.org/fibo/red/be/partnerships/partnerships/">
    <!ENTITY fibo-be-oac-opty "http://spec.edmcouncil.org/fibo/red/be/ownership-and-control/ownership-parties/">
    <!ENTITY fibo-be-oac-cpty "http://spec.edmcouncil.org/fibo/red/be/ownership-and-control/control-parties/">
]>

<rdf:RDF xmlns:xsd="http://www.w3.org/2001/XMLSchema#"
         xmlns:sm="http://www.omg.org/techprocess/ab/SpecificationMetadata/"
         xmlns:xs="http://www.w3.org/2001/XMLSchema"
         xmlns:fibo-fnd-utl-av="http://www.omg.org/spec/EDMC-FIBO/FND/Utilities/AnnotationVocabulary/"
         xmlns:rdf="http://www.w3.org/1999/02/22-rdf-syntax-ns#"
         xmlns:rdfs="http://www.w3.org/2000/01/rdf-schema#"
         xmlns:owl="http://www.w3.org/2002/07/owl#"
         xmlns:skos="http://www.w3.org/2004/02/skos/core#"
         xmlns:dc="http://purl.org/dc/terms/"
         xml:base="http://spec.edmcouncil.org/fibo/red/be/ownership-control-ext/control-parties-extras/">

   <owl:Ontology rdf:about="http://spec.edmcouncil.org/fibo/red/be/ownership-control-ext/control-parties-extras/">
      <owl:imports rdf:resource="http://spec.edmcouncil.org/fibo/red/fnd/agreements/contracts/"/>
      <owl:imports rdf:resource="http://spec.edmcouncil.org/fibo/red/fnd/parties/parties/"/>
      <owl:imports rdf:resource="http://spec.edmcouncil.org/fibo/red/be/legal-entities/formal-business-organizations/"/>
      <owl:imports rdf:resource="http://spec.edmcouncil.org/fibo/red/fnd/law/legal-capacities/"/>
      <owl:imports rdf:resource="http://spec.edmcouncil.org/fibo/red/be/partnerships/partnerships/"/>
      <owl:imports rdf:resource="http://spec.edmcouncil.org/fibo/red/be/ownership-and-control/ownership-parties/"/>
      <owl:imports rdf:resource="http://spec.edmcouncil.org/fibo/red/be/ownership-and-control/control-parties/"/>
   </owl:Ontology>


  <!--
    ///////////////////////////////////////////////////////////////////////////////////////
    //
    // Datatypes
    //
    ///////////////////////////////////////////////////////////////////////////////////////
    -->



  <!--
    ///////////////////////////////////////////////////////////////////////////////////////
    //
    // Object Properties
    //
    ///////////////////////////////////////////////////////////////////////////////////////
    -->


<owl:ObjectProperty rdf:about="&fibo-be-oacx-cptyx;contractualDeJureControlConferredBy">
      <rdfs:label>contractual de jure control conferred by</rdfs:label>
      <skos:definition>Contractual Control is conferred by some contract in which one party agrees to confer some degree and type of control upon the other party to that contract.</skos:definition>
      <rdfs:subPropertyOf rdf:resource="&fibo-fnd-law-lcap;isConferredBy"/>
      <rdfs:domain rdf:resource="&fibo-be-oac-cpty;ContractualControl"/>
      <rdfs:range rdf:resource="&fibo-be-oacx-cptyx;ControlRelatedContract"/>
   </owl:ObjectProperty>

   <owl:ObjectProperty rdf:about="&fibo-be-oacx-cptyx;deJureControllingInterestPartyHasIdentity">
      <rdfs:label>de jure controlling interest party has identity</rdfs:label>
      <skos:definition>That which performs the role of De Jure Controlling Party.</skos:definition>
      <rdfs:subPropertyOf rdf:resource="&fibo-fnd-pty-pty;hasIdentity"/>
      <rdfs:domain rdf:resource="&fibo-be-oac-cpty;DeJureControllingInterestParty"/>
      <rdfs:range rdf:resource="&fibo-fnd-pty-pty;IndependentParty"/>
   </owl:ObjectProperty>

   <owl:ObjectProperty rdf:about="&fibo-be-oacx-cptyx;entityControllingPartyIdentity">
      <rdfs:label>entity controlling party identity</rdfs:label>
      <skos:definition>That which is able to be the Entity Controlling Party. Scope Note: It is assumed that since control follows from some form of ownership or contractual instrument, that the range of entities which may fulfil this party role is the same as that for entity ownership, namely "Involved Party"; that is, a logical union of natural persons, legal persons and formal organizations.</skos:definition>
      <rdfs:subPropertyOf rdf:resource="&fibo-fnd-pty-pty;hasIdentity"/>
      <rdfs:domain rdf:resource="&fibo-be-oac-cpty;EntityControllingParty"/>
      <rdfs:range rdf:resource="&fibo-fnd-pty-pty;IndependentParty"/>
   </owl:ObjectProperty>

   <owl:ObjectProperty rdf:about="&fibo-be-oacx-cptyx;generalPartnerExercises">
      <rdfs:label>general partner exercises</rdfs:label>
      <skos:definition>The General Partner exercises control as a result of holding General Partner equity, which is therefore a form of constitutional control of the entity.</skos:definition>
      <rdfs:subPropertyOf rdf:resource="&fibo-be-oac-cpty;holdsSomeInstrumentOfDeJureControl"/>
      <rdfs:domain rdf:resource="&fibo-be-ptr-ptr;GeneralPartner"/>
      <rdfs:range rdf:resource="&fibo-be-oac-cpty;ConstitutionalDeJureControl"/>
   </owl:ObjectProperty>

   <owl:ObjectProperty rdf:about="&fibo-be-oacx-cptyx;exercisesMajorityOf">
      <rdfs:label>exercises majority of</rdfs:label>
      <skos:definition>Exercises, either alone or in equal degree with other such parties, majority De Facto Control over the entity in respect of which this party is defined.</skos:definition>
      <rdfs:subPropertyOf rdf:resource="&fibo-be-oac-cpty;hasDegreeOfControl"/>
      <rdfs:domain rdf:resource="&fibo-be-oac-cpty;MajorityControllingParty"/>
      <rdfs:range rdf:resource="&fibo-be-oac-cpty;DegreeOfControl"/>
   </owl:ObjectProperty>

   <owl:ObjectProperty rdf:about="&fibo-be-oacx-cptyx;effectivelyExercises">
      <rdfs:label>effectively exercises</rdfs:label>
      <skos:definition>The Investment Owning Party effectively exercises some degree of de facto control as a result of their interest in the entity.</skos:definition>
      <rdfs:subPropertyOf rdf:resource="&fibo-be-oac-cpty;holdsSomeMeansOfDeFactoControl"/>
      <rdfs:domain rdf:resource="&fibo-be-oac-opty;Investor"/>
      <rdfs:range rdf:resource="&fibo-be-oac-cpty;InvestmentBasedDeFactoControl"/>
   </owl:ObjectProperty>

   <owl:ObjectProperty rdf:about="&fibo-be-oacx-cptyx;exercisesSomeDegreeOfControlOver">
      <rdfs:label>exercises some degree of control over</rdfs:label>
      <rdfs:domain rdf:resource="&fibo-be-oac-cpty;EntityControllingParty"/>
      <rdfs:range rdf:resource="&fibo-be-le-fbo;FormallyConstitutedOrganization"/>
      <owl:inverseOf rdf:resource="&fibo-be-oac-cpty;isControlledToSomeDegreeBy"/>
   </owl:ObjectProperty>

   <owl:ObjectProperty rdf:about="&fibo-be-oacx-cptyx;hasDeFactoControllingInterestParty">
      <rdfs:label>has de facto controlling interest party</rdfs:label>
      <skos:definition>Some party which exercises some de facto control over the Formal Organization.</skos:definition>
      <rdfs:subPropertyOf rdf:resource="&fibo-be-oac-cpty;hasControllingInterestParty"/>
      <rdfs:domain rdf:resource="&fibo-be-le-fbo;FormallyConstitutedOrganization"/>
      <rdfs:range rdf:resource="&fibo-be-oac-cpty;DeFactoControllingInterestParty"/>
   </owl:ObjectProperty>

   <owl:ObjectProperty rdf:about="&fibo-be-oacx-cptyx;hasDeJureControllingInterestParty">
      <rdfs:label>has de jure controlling interest party</rdfs:label>
      <skos:definition>The Formal Organization is legally controlled in some way by some de jure controlling party, that is some entity which exercises legally based control.</skos:definition>
      <rdfs:subPropertyOf rdf:resource="&fibo-be-oac-cpty;hasControllingInterestParty"/>
      <rdfs:domain rdf:resource="&fibo-be-le-fbo;FormallyConstitutedOrganization"/>
      <rdfs:range rdf:resource="&fibo-be-oac-cpty;DeJureControllingInterestParty"/>
   </owl:ObjectProperty>


  <!--
    ///////////////////////////////////////////////////////////////////////////////////////
    //
    // Data Properties
    //
    ///////////////////////////////////////////////////////////////////////////////////////
    -->



  <!--
    ///////////////////////////////////////////////////////////////////////////////////////
    //
    // Annotation Properties
    //
    ///////////////////////////////////////////////////////////////////////////////////////
    -->



  <!--
    ///////////////////////////////////////////////////////////////////////////////////////
    //
    // Classes
    //
    ///////////////////////////////////////////////////////////////////////////////////////
    -->


<owl:Class rdf:about="&fibo-be-oacx-cptyx;ControlRelatedContract">
      <rdfs:label>control related contract</rdfs:label>
      <skos:definition>A contract in which one party agrees to confer some degree and type of control upon the other party to that contract.</skos:definition>
      <rdfs:subClassOf rdf:resource="&fibo-fnd-agr-ctr;Contract"/>
   </owl:Class>


  <!--
    ///////////////////////////////////////////////////////////////////////////////////////
    //
    // Individuals
    //
    ///////////////////////////////////////////////////////////////////////////////////////
    -->


</rdf:RDF>