<?xml version="1.0" encoding="UTF-8"?>
<rdf:RDF xmlns:xsd="http://www.w3.org/2001/XMLSchema#"
         xmlns:sm="http://www.omg.org/techprocess/ab/SpecificationMetadata/"
         xmlns:fibo-fnd-utl-av="http://www.omg.org/spec/EDMC-FIBO/FND/Utilities/AnnotationVocabulary/"
         xmlns:rdf="http://www.w3.org/1999/02/22-rdf-syntax-ns#"
         xmlns:rdfs="http://www.w3.org/2000/01/rdf-schema#"
         xmlns:owl="http://www.w3.org/2002/07/owl#"
         xmlns:skos="http://www.w3.org/2004/02/skos/core#"
         xmlns:dc="http://purl.org/dc/terms/"
         xml:base="http://www.edmcouncil.org/spec/EDMC-SR/FND/Transactions/TransactionsExtended/">

   <owl:Ontology rdf:about="http://www.edmcouncil.org/spec/EDMC-SR/FND/Transactions/TransactionsExtended/">
      <owl:imports rdf:resource="http://www.edmcouncil.org/spec/EDMC-SR/FND/Transactions/REATransactions/"/>
   </owl:Ontology>

   <!--Datatypes-->

<!--Object Properties-->

<owl:ObjectProperty rdf:about="http://www.edmcouncil.org/spec/EDMC-SR/FND/Transactions/TransactionsExtended/governs">
      <skos:definition>The contractual relationship defined by the master agreement.</skos:definition>
      <rdfs:domain rdf:resource="http://www.edmcouncil.org/spec/EDMC-SR/FND/Transactions/TransactionsExtended/MasterAgreement"/>
      <rdfs:range rdf:resource="http://www.omg.org/spec/EDMC-SR/FND/Agreements/Contracts/ContractualRelationship"/>
   </owl:ObjectProperty>

   <owl:ObjectProperty rdf:about="http://www.edmcouncil.org/spec/EDMC-SR/FND/Transactions/TransactionsExtended/governedBy">
      <rdfs:domain rdf:resource="http://www.edmcouncil.org/spec/EDMC-SR/FND/Transactions/TransactionsExtended/CoveredTransaction"/>
      <rdfs:range rdf:resource="http://www.edmcouncil.org/spec/EDMC-SR/FND/Transactions/TransactionsExtended/MasterAgreement"/>
   </owl:ObjectProperty>

   <!--Data Properties-->

<!--Annotation Properties-->

<!--Classes-->

<owl:Class rdf:about="http://www.edmcouncil.org/spec/EDMC-SR/FND/Transactions/TransactionsExtended/ContractuallyDefinedBenefit">
      <rdfs:label>Contractually Defined Benefit</rdfs:label>
      <skos:definition>Some benefit from one party to the other party, defined in contractual terms.</skos:definition>
      <skos:editorialNote>This could for example be a contractual promise of future cash flows such as dividends on a specific instrument.</skos:editorialNote>
      <rdfs:subClassOf rdf:resource="http://www.edmcouncil.org/spec/EDMC-SR/FND/Relative/EconomicResources/EconomicResource"/>
   </owl:Class>

   <owl:Class rdf:about="http://www.edmcouncil.org/spec/EDMC-SR/FND/Transactions/TransactionsExtended/CoveredTransaction">
      <rdfs:label>Covered Transaction</rdfs:label>
      <skos:definition>A transaction covered by some Master Agreement.</skos:definition>
      <skos:editorialNote>The Master Agreement sets out the terms and conditions under which these transactions are to take place between the parties. These are Over the Counter transactions, including OTC Derivatives.</skos:editorialNote>
      <rdfs:subClassOf rdf:resource="http://www.edmcouncil.org/spec/EDMC-SR/FND/Transactions/REATransactions/ContractualTransaction"/>
   </owl:Class>

   <owl:Class rdf:about="http://www.edmcouncil.org/spec/EDMC-SR/FND/Transactions/TransactionsExtended/MasterAgreement">
      <rdfs:label>Master Agreement</rdfs:label>
      <skos:definition>A legal contract which is deemed to apply to a number of future activities between the parties thereto and having force over future agreements or contracts to be brought into effect between those parties.</skos:definition>
      <rdfs:subClassOf rdf:resource="http://www.omg.org/spec/EDMC-SR/FND/Agreements/Contracts/WrittenContract"/>
   </owl:Class>

   <!--Individuals-->

</rdf:RDF>