<?xml version="1.0" encoding="UTF-8"?>
  
<!DOCTYPE rdf:RDF [
    <!ENTITY fibo-fnd-plc-cty "http://spec.edmcouncil.org/fibo/red/fnd/places/countries/">
    <!ENTITY fibo-fnd-soc-soc "http://spec.edmcouncil.org/fibo/red/fnd/social-constructs/social-constructs/">
    <!ENTITY fibo-fnd-utl-bt "http://spec.edmcouncil.org/fibo/red/fnd/utilities/business-facing-types/">
    <!ENTITY fibo-fnd-plc-loc "http://spec.edmcouncil.org/fibo/red/fnd/places/locations/">
    <!ENTITY fibo-fnd-plcx-gph "http://spec.edmcouncil.org/fibo/red/fnd/places-ext/geophysical/">
]>

<rdf:RDF xmlns:xsd="http://www.w3.org/2001/XMLSchema#"
         xmlns:sm="http://www.omg.org/techprocess/ab/SpecificationMetadata/"
         xmlns:xs="http://www.w3.org/2001/XMLSchema"
         xmlns:fibo-fnd-utl-av="http://www.omg.org/spec/EDMC-FIBO/FND/Utilities/AnnotationVocabulary/"
         xmlns:rdf="http://www.w3.org/1999/02/22-rdf-syntax-ns#"
         xmlns:rdfs="http://www.w3.org/2000/01/rdf-schema#"
         xmlns:owl="http://www.w3.org/2002/07/owl#"
         xmlns:skos="http://www.w3.org/2004/02/skos/core#"
         xmlns:dc="http://purl.org/dc/terms/"
         xml:base="http://spec.edmcouncil.org/fibo/red/fnd/places/countries/">

   <owl:Ontology rdf:about="http://spec.edmcouncil.org/fibo/red/fnd/places/countries/">
      <owl:imports rdf:resource="http://spec.edmcouncil.org/fibo/red/fnd/social-constructs/social-constructs/"/>
      <owl:imports rdf:resource="http://spec.edmcouncil.org/fibo/red/fnd/utilities/business-facing-types/"/>
      <owl:imports rdf:resource="http://spec.edmcouncil.org/fibo/red/fnd/places/locations/"/>
      <owl:imports rdf:resource="http://spec.edmcouncil.org/fibo/red/fnd/places-ext/geophysical/"/>
   </owl:Ontology>


  <!--
    ///////////////////////////////////////////////////////////////////////////////////////
    //
    // Datatypes
    //
    ///////////////////////////////////////////////////////////////////////////////////////
    -->



  <!--
    ///////////////////////////////////////////////////////////////////////////////////////
    //
    // Object Properties
    //
    ///////////////////////////////////////////////////////////////////////////////////////
    -->



  <!--
    ///////////////////////////////////////////////////////////////////////////////////////
    //
    // Data Properties
    //
    ///////////////////////////////////////////////////////////////////////////////////////
    -->


<owl:DatatypeProperty rdf:about="&fibo-fnd-plc-cty;abbreviation">
      <rdfs:label>abbreviation</rdfs:label>
      <skos:definition>The abbreviation by which the state or province is known in its country, e.g. CA, BC.</skos:definition>
      <rdfs:range rdf:resource="&fibo-fnd-utl-bt;text"/>
   </owl:DatatypeProperty>

   <owl:DatatypeProperty rdf:about="&fibo-fnd-plc-cty;designation">
      <rdfs:label>designation</rdfs:label>
      <skos:definition>What the federal unit is called in this country, e.g. State, Province, Canton.</skos:definition>
      <rdfs:range rdf:resource="&fibo-fnd-utl-bt;text"/>
   </owl:DatatypeProperty>

   <owl:DatatypeProperty rdf:about="&fibo-fnd-plc-cty;officialName">
      <rdfs:label>official name</rdfs:label>
      <skos:definition>The official name of the country, e.g. "People's Republic of ..." Note that the common name for the country is the "Name" term inherited from the Geographical Entity.</skos:definition>
      <rdfs:range rdf:resource="&fibo-fnd-utl-bt;text"/>
   </owl:DatatypeProperty>


  <!--
    ///////////////////////////////////////////////////////////////////////////////////////
    //
    // Annotation Properties
    //
    ///////////////////////////////////////////////////////////////////////////////////////
    -->



  <!--
    ///////////////////////////////////////////////////////////////////////////////////////
    //
    // Classes
    //
    ///////////////////////////////////////////////////////////////////////////////////////
    -->


<owl:Class rdf:about="&fibo-fnd-plc-cty;FederalCapitalArea">
      <rdfs:label>federal capital area</rdfs:label>
      <skos:definition>The capital administrative region of a country which is a federation, if the physical area of this region does not form a part of any of the states or provinces which make up the federal country.</skos:definition>
      <rdfs:subClassOf rdf:resource="&fibo-fnd-plc-cty;GeopoliticalEntity"/>
   </owl:Class>

   <owl:Class rdf:about="&fibo-fnd-plc-cty;FederalState">
      <rdfs:label>federal state</rdfs:label>
      <skos:definition>A self-governing geopolitical entity which forms part of a wider geopolitical entity recognized as a country. This type of entity, variously referred to as a state, province or canton, has a level of self government including its own legal system and court jurisdiction, but cedes a level of autonomy to the federation of which it forms a part.</skos:definition>
   </owl:Class>

   <owl:Class rdf:about="&fibo-fnd-plc-cty;GeopoliticalEntity">
      <rdfs:label>geopolitical entity</rdfs:label>
      <rdfs:subClassOf rdf:resource="&fibo-fnd-plc-loc;PhysicalLocation"/>
      <rdfs:subClassOf rdf:resource="&fibo-fnd-soc-soc;SocialConstruct"/>
   </owl:Class>

   <owl:Class rdf:about="&fibo-fnd-plc-cty;Country">
      <rdfs:label>country</rdfs:label>
   </owl:Class>

   <owl:Class rdf:about="&fibo-fnd-plc-cty;UrbanCenter">
      <rdfs:label>urban center</rdfs:label>
      <skos:definition>a large and densely populated urban area</skos:definition>
      <rdfs:subClassOf rdf:resource="&fibo-fnd-plcx-gph;GeographicalArea"/>
   </owl:Class>


  <!--
    ///////////////////////////////////////////////////////////////////////////////////////
    //
    // Individuals
    //
    ///////////////////////////////////////////////////////////////////////////////////////
    -->


</rdf:RDF>