<?xml version="1.0" encoding="UTF-8"?>
<rdf:RDF xmlns:xsd="http://www.w3.org/2001/XMLSchema#"
         xmlns:sm="http://www.omg.org/techprocess/ab/SpecificationMetadata/"
         xmlns:fibo-fnd-utl-av="http://www.omg.org/spec/EDMC-FIBO/FND/Utilities/AnnotationVocabulary/"
         xmlns:rdf="http://www.w3.org/1999/02/22-rdf-syntax-ns#"
         xmlns:rdfs="http://www.w3.org/2000/01/rdf-schema#"
         xmlns:owl="http://www.w3.org/2002/07/owl#"
         xmlns:skos="http://www.w3.org/2004/02/skos/core#"
         xmlns:dc="http://purl.org/dc/terms/"
         xml:base="http://www.omg.org/spec/EDMC-FIBO/DER/ExchangeTradedDerivatives/OptionsExchanges/">

   <owl:Ontology rdf:about="http://www.omg.org/spec/EDMC-FIBO/DER/ExchangeTradedDerivatives/OptionsExchanges/">
      <owl:imports rdf:resource="http://www.omg.org/spec/EDMC-FIBO/DER/ExchangeTradedDerivatives/DerivativesStandardizedTerms/"/>
   </owl:Ontology>

   <!--Datatypes-->

<!--Object Properties-->

<owl:ObjectProperty rdf:about="http://www.omg.org/spec/EDMC-FIBO/DER/ExchangeTradedDerivatives/OptionsExchanges/canBecome">
      <rdfs:domain rdf:resource="http://www.omg.org/spec/EDMC-FIBO/DER/ExchangeTradedDerivatives/OptionsExchanges/TradingParticipant"/>
      <rdfs:range rdf:resource="http://www.omg.org/spec/EDMC-FIBO/DER/ExchangeTradedDerivatives/OptionsExchanges/ClearingParticipant"/>
   </owl:ObjectProperty>

   <owl:ObjectProperty rdf:about="http://www.omg.org/spec/EDMC-FIBO/DER/ExchangeTradedDerivatives/OptionsExchanges/mayBe">
      <rdfs:domain rdf:resource="http://www.omg.org/spec/EDMC-FIBO/DER/ExchangeTradedDerivatives/OptionsExchanges/TradingParticipant"/>
      <rdfs:range rdf:resource="http://www.omg.org/spec/EDMC-FIBO/DER/ExchangeTradedDerivatives/OptionsExchanges/DerivativesBroker"/>
   </owl:ObjectProperty>

   <!--Data Properties-->

<!--Annotation Properties-->

<!--Classes-->

<owl:Class rdf:about="http://www.omg.org/spec/EDMC-FIBO/DER/ExchangeTradedDerivatives/OptionsExchanges/ClearingParticipant">
      <rdfs:label>Clearing Participant</rdfs:label>
      <skos:definition>People who are members of the exchange who are allowed to clear the trades. There are various categories of entities which are participating in this full process: FTrading Member Clearing Member Entity which does both for itself (not professionally carrying out the clearing for other</skos:definition>
      <rdfs:subClassOf rdf:resource="http://www.omg.org/spec/EDMC-FIBO/DER/ExchangeTradedDerivatives/OptionsExchanges/TradingParticipant"/>
   </owl:Class>

   <owl:Class rdf:about="http://www.omg.org/spec/EDMC-FIBO/DER/ExchangeTradedDerivatives/OptionsExchanges/DerivativesBroker">
      <rdfs:label>Derivatives Broker</rdfs:label>
      <skos:definition>A party which is party to the transaction between entities which are not on the Derivatives Exchange. The Broker is then also a member of the Exchange (see Trading PArticipant), and in this context is the one who carries out the deals on the exchange, and who settles his margin daily. These may poarticipate in the OTC market also, where they just get a fee for introdiucing them. In formal exchanges, the Broker is doing th edeal, and the fact that the deal is passed on to others is a separate transaction, which they are also party to.</skos:definition>
   </owl:Class>

   <owl:Class rdf:about="http://www.omg.org/spec/EDMC-FIBO/DER/ExchangeTradedDerivatives/OptionsExchanges/MarginAccount">
      <rdfs:label>Margin Account</rdfs:label>
      <skos:definition>Account held at a Derivatives Exchange by a participant in that exchange.</skos:definition>
      <rdfs:subClassOf rdf:resource="http://www.edmcouncil.org/spec/EDMC-SR/FND/Accounting/AccountsMain/Account"/>
   </owl:Class>

   <owl:Class rdf:about="http://www.omg.org/spec/EDMC-FIBO/DER/ExchangeTradedDerivatives/OptionsExchanges/OptionsExchangeParticipant">
      <rdfs:label>Options Exchange Participant</rdfs:label>
      <rdfs:subClassOf rdf:resource="http://www.omg.org/spec/EDMC-SR/FND/Parties/Parties/PartyInRole"/>
   </owl:Class>

   <owl:Class rdf:about="http://www.omg.org/spec/EDMC-FIBO/DER/ExchangeTradedDerivatives/OptionsExchanges/OptionsListing">
      <rdfs:label>Options Listing</rdfs:label>
      <skos:definition>A listing of an options instrument on a derivatives exchange. The listing is a product of the individual exchange.</skos:definition>
      <skos:editorialNote>This term sdoes not exist. If there was a listing of something that was an option, it would be a warrant. Review: We agreed to come back to this definition and verify whether it means the same as listing in the equities sense .</skos:editorialNote>
      <rdfs:subClassOf rdf:resource="http://www.omg.org/spec/EDMC-FIBO/DER/ExchangeTradedDerivatives/DerivativesStandardizedTerms/DerivativesListing"/>
   </owl:Class>

   <owl:Class rdf:about="http://www.omg.org/spec/EDMC-FIBO/DER/ExchangeTradedDerivatives/OptionsExchanges/TradingParticipant">
      <rdfs:label>Trading Participant</rdfs:label>
      <rdfs:subClassOf rdf:resource="http://www.omg.org/spec/EDMC-FIBO/DER/ExchangeTradedDerivatives/OptionsExchanges/OptionsExchangeParticipant"/>
   </owl:Class>

   <!--Individuals-->

</rdf:RDF>