<?xml version="1.0" encoding="UTF-8"?>
  
<!DOCTYPE rdf:RDF [
    <!ENTITY fibo-be-oac-cctl "http://spec.edmcouncil.org/fibo/red/be/ownership-and-control/corporate-control/">
    <!ENTITY fibo-be-oac-cpty "http://spec.edmcouncil.org/fibo/red/be/ownership-and-control/control-parties/">
    <!ENTITY fibo-be-oac-cown "http://spec.edmcouncil.org/fibo/red/be/ownership-and-control/corporate-ownership/">
    <!ENTITY fibo-fnd-oac-ctl "http://spec.edmcouncil.org/fibo/red/fnd/ownership-and-control/control/">
    <!ENTITY fibo-be-le-fbo "http://spec.edmcouncil.org/fibo/red/be/legal-entities/formal-business-organizations/">
    <!ENTITY fibo-be-oac-opty "http://spec.edmcouncil.org/fibo/red/be/ownership-and-control/ownership-parties/">
    <!ENTITY fibo-sec-eq-eqi "http://spec.edmcouncil.org/fibo/red/sec/equities/equity-instruments/">
    <!ENTITY fibo-be-oacx-optyx "http://spec.edmcouncil.org/fibo/red/be/ownership-control-ext/ownership-parties-extras/">
    <!ENTITY fibo-fnd-pty-pty "http://spec.edmcouncil.org/fibo/red/fnd/parties/parties/">
    <!ENTITY fibo-be-corp-corp "http://spec.edmcouncil.org/fibo/red/be/corporations/corporations/">
]>

<rdf:RDF xmlns:xsd="http://www.w3.org/2001/XMLSchema#"
         xmlns:sm="http://www.omg.org/techprocess/ab/SpecificationMetadata/"
         xmlns:xs="http://www.w3.org/2001/XMLSchema"
         xmlns:fibo-fnd-utl-av="http://www.omg.org/spec/EDMC-FIBO/FND/Utilities/AnnotationVocabulary/"
         xmlns:rdf="http://www.w3.org/1999/02/22-rdf-syntax-ns#"
         xmlns:rdfs="http://www.w3.org/2000/01/rdf-schema#"
         xmlns:owl="http://www.w3.org/2002/07/owl#"
         xmlns:skos="http://www.w3.org/2004/02/skos/core#"
         xmlns:dc="http://purl.org/dc/terms/"
         xml:base="http://spec.edmcouncil.org/fibo/red/be/ownership-and-control/corporate-control/">

   <owl:Ontology rdf:about="http://spec.edmcouncil.org/fibo/red/be/ownership-and-control/corporate-control/">
      <owl:imports rdf:resource="http://spec.edmcouncil.org/fibo/red/be/ownership-and-control/control-parties/"/>
      <owl:imports rdf:resource="http://spec.edmcouncil.org/fibo/red/be/ownership-and-control/corporate-ownership/"/>
      <owl:imports rdf:resource="http://spec.edmcouncil.org/fibo/red/fnd/ownership-and-control/control/"/>
      <owl:imports rdf:resource="http://spec.edmcouncil.org/fibo/red/be/legal-entities/formal-business-organizations/"/>
      <owl:imports rdf:resource="http://spec.edmcouncil.org/fibo/red/be/ownership-and-control/ownership-parties/"/>
      <owl:imports rdf:resource="http://spec.edmcouncil.org/fibo/red/sec/equities/equity-instruments/"/>
      <owl:imports rdf:resource="http://spec.edmcouncil.org/fibo/red/be/ownership-control-ext/ownership-parties-extras/"/>
      <owl:imports rdf:resource="http://spec.edmcouncil.org/fibo/red/fnd/parties/parties/"/>
      <owl:imports rdf:resource="http://spec.edmcouncil.org/fibo/red/be/corporations/corporations/"/>
   </owl:Ontology>


  <!--
    ///////////////////////////////////////////////////////////////////////////////////////
    //
    // Datatypes
    //
    ///////////////////////////////////////////////////////////////////////////////////////
    -->



  <!--
    ///////////////////////////////////////////////////////////////////////////////////////
    //
    // Object Properties
    //
    ///////////////////////////////////////////////////////////////////////////////////////
    -->


<owl:ObjectProperty rdf:about="&fibo-be-oac-cctl;controlledCompanyIdentity">
      <rdfs:label>controlled company identity</rdfs:label>
      <skos:definition>That Formal Organization which is identified as a controlled company.</skos:definition>
      <rdfs:subPropertyOf rdf:resource="&fibo-fnd-pty-pty;hasIdentity"/>
      <rdfs:domain rdf:resource="&fibo-be-oac-cctl;ControlledCompany"/>
      <rdfs:range rdf:resource="&fibo-be-le-fbo;FormallyConstitutedOrganization"/>
   </owl:ObjectProperty>

   <owl:ObjectProperty rdf:about="&fibo-be-oac-cctl;incorporatedCompanyHasControllingInterestParty">
      <rdfs:label>incorporated company has controlling interest party</rdfs:label>
      <skos:definition>Some control of the Incorporated Company is wielded by some Voting Shareholder.</skos:definition>
      <rdfs:subPropertyOf rdf:resource="&fibo-be-oac-cpty;hasControllingInterestParty"/>
      <rdfs:domain rdf:resource="&fibo-be-corp-corp;IncorporatedCompany"/>
      <rdfs:range rdf:resource="&fibo-be-oac-cctl;VotingShareholder"/>
   </owl:ObjectProperty>

   <owl:ObjectProperty rdf:about="&fibo-be-oac-cctl;incprporatedCompanyHasSignificantControllingInterestCompany">
      <rdfs:label>incprporated company has significant controlling interest company</rdfs:label>
      <rdfs:subPropertyOf rdf:resource="&fibo-be-oac-cpty;hasSignificantControllingInterstParty"/>
      <rdfs:domain rdf:resource="&fibo-be-corp-corp;IncorporatedCompany"/>
      <rdfs:range rdf:resource="&fibo-be-oac-cctl;SignificantShareholdingCompany"/>
      <owl:inverseOf rdf:resource="&fibo-be-oac-cctl;holdsSignificantControllingInterestIn"/>
   </owl:ObjectProperty>

   <owl:ObjectProperty rdf:about="&fibo-be-oac-cctl;hasVotingRights">
      <rdfs:label>has voting rights</rdfs:label>
      <skos:definition>The Voting Shareholder holds certain Voting Rights as a consequence of their holding of those shares.</skos:definition>
      <rdfs:subPropertyOf rdf:resource="&fibo-be-oac-cctl;holdsSome"/>
      <rdfs:domain rdf:resource="&fibo-be-oac-cctl;VotingShareholder"/>
      <rdfs:range rdf:resource="&fibo-sec-eq-eqi;VotingRight"/>
   </owl:ObjectProperty>

   <owl:ObjectProperty rdf:about="&fibo-be-oac-cctl;holdsSome">
      <rdfs:label>holds some</rdfs:label>
      <skos:definition>Voting Shareholder is the holder of some Voting Share.</skos:definition>
      <rdfs:domain rdf:resource="&fibo-be-oac-cctl;VotingShareholder"/>
      <rdfs:range rdf:resource="&fibo-sec-eq-eqi;VotingShare"/>
   </owl:ObjectProperty>

   <owl:ObjectProperty rdf:about="&fibo-be-oac-cctl;votingShareholdingCompanyHasIdentity">
      <rdfs:label>voting shareholding company has identity</rdfs:label>
      <skos:definition>The Shareholding Company is a Formal Organization.</skos:definition>
      <rdfs:subPropertyOf rdf:resource="&fibo-fnd-pty-pty;hasIdentity"/>
      <rdfs:subPropertyOf rdf:resource="&fibo-be-oacx-optyx;entityOwningPartyIdentity"/>
      <rdfs:domain rdf:resource="&fibo-be-oac-cctl;VotingShareholdingCompany"/>
      <rdfs:range rdf:resource="&fibo-be-le-fbo;FormallyConstitutedOrganization"/>
   </owl:ObjectProperty>

   <owl:ObjectProperty rdf:about="&fibo-be-oac-cctl;votingShareholdingCompanyHoldsControllingInterestIn">
      <rdfs:label>voting shareholding company holds controlling interest in</rdfs:label>
      <skos:definition>A registered company which is a part or subsidiary of the Incorporated Company in the same or another Jurisdiction.</skos:definition>
      <rdfs:subPropertyOf rdf:resource="&fibo-be-oac-cctl;holdsControllingInterestIn"/>
      <rdfs:domain rdf:resource="&fibo-be-oac-cctl;VotingShareholdingCompany"/>
      <rdfs:range rdf:resource="&fibo-be-corp-corp;IncorporatedCompany"/>
   </owl:ObjectProperty>

   <owl:ObjectProperty rdf:about="&fibo-be-oac-cctl;heldBy">
      <rdfs:label>held by</rdfs:label>
      <skos:definition>The holder of the Voting Shares, that is the party of which this is the shareholding and which therefore enjoys the voting rights thereof.</skos:definition>
      <rdfs:subPropertyOf rdf:resource="&fibo-be-oac-cown;heldBy"/>
      <rdfs:domain rdf:resource="&fibo-be-oac-cctl;VotingShareholding"/>
      <rdfs:range rdf:resource="&fibo-be-oac-cctl;VotingShareholder"/>
   </owl:ObjectProperty>

   <owl:ObjectProperty rdf:about="&fibo-be-oac-cctl;hasAffiliarte">
      <rdfs:label>has affiliarte</rdfs:label>
      <skos:definition>Ownership between some minimum percentage and majority holding. That minimum percentage is determined in local law and may be for example 10% or 25%.</skos:definition>
      <rdfs:subPropertyOf rdf:resource="&fibo-be-oac-cpty;hasControllingInterestParty"/>
      <rdfs:domain rdf:resource="&fibo-be-corp-corp;IncorporatedCompany"/>
      <rdfs:range rdf:resource="&fibo-be-oac-cctl;Affiliate"/>
   </owl:ObjectProperty>

   <owl:ObjectProperty rdf:about="&fibo-be-oac-cctl;hasControllingInterestPartyVotingShareholdingCompany">
      <rdfs:label>has controlling interest party voting shareholding company</rdfs:label>
      <rdfs:subPropertyOf rdf:resource="&fibo-be-oac-cctl;incorporatedCompanyHasControllingInterestParty"/>
      <rdfs:domain rdf:resource="&fibo-be-corp-corp;IncorporatedCompany"/>
      <rdfs:range rdf:resource="&fibo-be-oac-cctl;VotingShareholdingCompany"/>
      <owl:inverseOf rdf:resource="&fibo-be-oac-cctl;votingShareholdingCompanyHoldsControllingInterestIn"/>
   </owl:ObjectProperty>

   <owl:ObjectProperty rdf:about="&fibo-be-oac-cctl;hasDomesticUltimateParent">
      <rdfs:label>has domestic ultimate parent</rdfs:label>
      <skos:definition>The organization which is recognized as the ultimate parent of the company within the country or jurisdiction of incorporation. This relationship may or may not be present, i.e. in the case of a company which has no parent.</skos:definition>
      <rdfs:subPropertyOf rdf:resource="&fibo-be-oac-cpty;hasMajorityControllingParty"/>
      <rdfs:domain rdf:resource="&fibo-be-corp-corp;IncorporatedCompany"/>
      <rdfs:range rdf:resource="&fibo-be-oac-cctl;DomesticUltimateParent"/>
   </owl:ObjectProperty>

   <owl:ObjectProperty rdf:about="&fibo-be-oac-cctl;hasGlobalUltimateParent">
      <rdfs:label>has global ultimate parent</rdfs:label>
      <skos:definition>The organization which is recognized as the ultimate parent of the company. This relationship may or may not be present, i.e. in the case of a company which has no parent.</skos:definition>
      <rdfs:subPropertyOf rdf:resource="&fibo-be-oac-cpty;hasMajorityControllingParty"/>
      <rdfs:domain rdf:resource="&fibo-be-corp-corp;IncorporatedCompany"/>
      <rdfs:range rdf:resource="&fibo-be-oac-cctl;GlobalUltimateParent"/>
   </owl:ObjectProperty>

   <owl:ObjectProperty rdf:about="&fibo-be-oac-cctl;hasMajorityControllingInterestParty">
      <rdfs:label>has majority controlling interest party</rdfs:label>
      <skos:definition>The parent organization of the company, if there is one.</skos:definition>
      <rdfs:subPropertyOf rdf:resource="&fibo-be-oac-cpty;hasSignificantControllingInterstParty"/>
      <rdfs:domain rdf:resource="&fibo-be-corp-corp;IncorporatedCompany"/>
      <rdfs:range rdf:resource="&fibo-be-oac-cctl;OverFiftyPercentControlingInterestCompany"/>
   </owl:ObjectProperty>

   <owl:ObjectProperty rdf:about="&fibo-be-oac-cctl;hasMajorityOwnedSubsidiary">
      <rdfs:label>has majority owned subsidiary</rdfs:label>
      <skos:definition>A company which is recognized as a majority owned subsidiary of this company. This is where there is above 50% (50% plus one share) ownership of the shares.</skos:definition>
      <rdfs:subPropertyOf rdf:resource="&fibo-be-oac-cctl;hasSubsidiary"/>
      <rdfs:domain rdf:resource="&fibo-be-corp-corp;IncorporatedCompany"/>
      <rdfs:range rdf:resource="&fibo-be-oac-cctl;WhollyOwnedSubsidiary"/>
   </owl:ObjectProperty>

   <owl:ObjectProperty rdf:about="&fibo-be-oac-cctl;hasSubsidiary">
      <rdfs:label>has subsidiary</rdfs:label>
      <skos:definition>The company has control over some company, which is identified as a Subsidiary by virtue of this.</skos:definition>
      <rdfs:domain rdf:resource="&fibo-be-corp-corp;IncorporatedCompany"/>
      <rdfs:range rdf:resource="&fibo-be-oac-cctl;Subsidiary"/>
   </owl:ObjectProperty>

   <owl:ObjectProperty rdf:about="&fibo-be-oac-cctl;holdsControllingInterestIn">
      <rdfs:label>holds controlling interest in</rdfs:label>
      <skos:definition>The shareholder holds some voting stake in the Incorporated Company, by means of their holding of voting shares.</skos:definition>
      <rdfs:subPropertyOf rdf:resource="&fibo-be-oac-opty;holdsAnInterestIn"/>
      <rdfs:domain rdf:resource="&fibo-be-oac-cctl;VotingShareholder"/>
      <rdfs:range rdf:resource="&fibo-be-corp-corp;IncorporatedCompany"/>
   </owl:ObjectProperty>

   <owl:ObjectProperty rdf:about="&fibo-be-oac-cctl;holdsMajorityControllingInterestIn">
      <rdfs:label>holds majority controlling interest in</rdfs:label>
      <skos:definition>The Incorporated Company in which the party holds fifty percent or more of the voting share equity.</skos:definition>
      <rdfs:subPropertyOf rdf:resource="&fibo-be-oac-cctl;holdsControllingInterestIn"/>
      <rdfs:domain rdf:resource="&fibo-be-oac-cctl;VotingShareholder"/>
      <rdfs:range rdf:resource="&fibo-be-corp-corp;IncorporatedCompany"/>
   </owl:ObjectProperty>

   <owl:ObjectProperty rdf:about="&fibo-be-oac-cctl;holdsSignificantControllingInterestIn">
      <rdfs:label>holds significant controlling interest in</rdfs:label>
      <skos:definition>The Incorporated Company in which the party holds a significant proportion (but not fifty percent or more) of the voting share equity.</skos:definition>
      <rdfs:subPropertyOf rdf:resource="&fibo-be-oac-cctl;holdsControllingInterestIn"/>
      <rdfs:domain rdf:resource="&fibo-be-oac-cctl;VotingShareholder"/>
      <rdfs:range rdf:resource="&fibo-be-corp-corp;IncorporatedCompany"/>
   </owl:ObjectProperty>

   <owl:ObjectProperty rdf:about="&fibo-be-oac-cctl;exercisesEquityBasedDeJureControl">
      <rdfs:label>exercises equity based de jure control</rdfs:label>
      <skos:definition>A Voting Shareholder exercise some Equity Based de jure control in the entity for which they hold those shares.</skos:definition>
      <rdfs:subPropertyOf rdf:resource="&fibo-be-oac-cpty;holdsSomeInstrumentOfDeJureControl"/>
      <rdfs:domain rdf:resource="&fibo-be-oac-cctl;VotingShareholder"/>
      <rdfs:range rdf:resource="&fibo-be-oac-cpty;EquityBasedDeJureControl"/>
   </owl:ObjectProperty>

   <owl:ObjectProperty rdf:about="&fibo-be-oac-cctl;isWhollyOwnedBy">
      <rdfs:label>is wholly owned by</rdfs:label>
      <skos:definition>The Incorporated Company is totally owned and therefore wholly controlled by some Formal Organization having 100% ownership in it.</skos:definition>
      <rdfs:subPropertyOf rdf:resource="&fibo-be-oac-cctl;hasMajorityControllingInterestParty"/>
      <rdfs:subPropertyOf rdf:resource="&fibo-be-oac-cpty;hasTotalOwner"/>
      <rdfs:domain rdf:resource="&fibo-be-corp-corp;IncorporatedCompany"/>
      <rdfs:range rdf:resource="&fibo-be-oac-cctl;TotalControllingInterestCompany"/>
   </owl:ObjectProperty>


  <!--
    ///////////////////////////////////////////////////////////////////////////////////////
    //
    // Data Properties
    //
    ///////////////////////////////////////////////////////////////////////////////////////
    -->



  <!--
    ///////////////////////////////////////////////////////////////////////////////////////
    //
    // Annotation Properties
    //
    ///////////////////////////////////////////////////////////////////////////////////////
    -->



  <!--
    ///////////////////////////////////////////////////////////////////////////////////////
    //
    // Classes
    //
    ///////////////////////////////////////////////////////////////////////////////////////
    -->


<owl:Class rdf:about="&fibo-be-oac-cctl;.UnionClass.5">
      <owl:equivalentClass>
         <owl:Class>
            <owl:unionOf rdf:parseType="Collection">
               <owl:Class rdf:about="&fibo-be-oac-cctl;ControlledCompany"/>
               <owl:Class rdf:about="&fibo-fnd-oac-ctl;ControllingParty"/>
            </owl:unionOf>
         </owl:Class>
      </owl:equivalentClass>
   </owl:Class>

   <owl:Class rdf:about="&fibo-be-oac-cctl;Affiliate">
      <rdfs:label>affiliate</rdfs:label>
   </owl:Class>

   <owl:Class rdf:about="&fibo-be-oac-cctl;ControlledCompany">
      <rdfs:label>controlled company</rdfs:label>
      <skos:definition>A company over which the Incorporated Company has some degree of control by way of ownership of voting shares.</skos:definition>
      <rdfs:subClassOf rdf:resource="&fibo-be-oac-cpty;ControlledParty"/>
   </owl:Class>

   <owl:Class rdf:about="&fibo-be-oac-cctl;DomesticUltimateParent">
      <rdfs:label>domestic ultimate parent</rdfs:label>
      <skos:definition>The organization which is recognized as the ultimate parent of the company within the country or jurisdiction of incorporation. This relationship may or may not be present, i.e. in the case of a company which has no parent.</skos:definition>
      <rdfs:subClassOf rdf:resource="&fibo-be-oac-cpty;MajorityControllingParty"/>
   </owl:Class>

   <owl:Class rdf:about="&fibo-be-oac-cctl;GlobalUltimateParent">
      <rdfs:label>global ultimate parent</rdfs:label>
      <skos:definition>The organization which is recognized as the ultimate parent of the company. This relationship may or may not be present, i.e. in the case of a company which has no parent.</skos:definition>
   </owl:Class>

   <owl:Class rdf:about="&fibo-be-oac-cctl;JointVenturePartner">
      <rdfs:label>joint venture partner</rdfs:label>
      <skos:definition>A party which has the role of Joint Venture Partner to some venture.</skos:definition>
      <rdfs:subClassOf rdf:resource="&fibo-be-oac-cpty;EntityControllingParty"/>
   </owl:Class>

   <owl:Class rdf:about="&fibo-be-oac-cctl;NonWhollyOwnedSubsidiary">
      <rdfs:label>non wholly owned subsidiary</rdfs:label>
      <skos:definition>A subsidiary which is not a wholly owned subsidiary.</skos:definition>
      <rdfs:subClassOf rdf:resource="&fibo-be-oac-cctl;Subsidiary"/>
   </owl:Class>

   <owl:Class rdf:about="&fibo-be-oac-cctl;OverFiftyPercentControlingInterestCompany">
      <rdfs:label>over fifty percent controling interest company</rdfs:label>
      <rdfs:subClassOf rdf:resource="&fibo-be-oac-cctl;VotingShareholdingCompany"/>
   </owl:Class>

   <owl:Class rdf:about="&fibo-be-oac-cctl;SignificantShareholdingCompany">
      <rdfs:label>significant shareholding company</rdfs:label>
      <skos:definition>A company which owns a significant voting stake in this company but not 50% or more.</skos:definition>
      <rdfs:subClassOf rdf:resource="&fibo-be-oac-cpty;SignificantControllingInterestParty"/>
   </owl:Class>

   <owl:Class rdf:about="&fibo-be-oac-cctl;Subsidiary">
      <rdfs:label>subsidiary</rdfs:label>
      <rdfs:subClassOf rdf:resource="&fibo-be-oac-cctl;ControlledCompany"/>
   </owl:Class>

   <owl:Class rdf:about="&fibo-be-oac-cctl;TotalControllingInterestCompany">
      <rdfs:label>total controlling interest company</rdfs:label>
      <skos:definition>Formal Organization having 100% ownership in the Incorporated Company so owned.</skos:definition>
      <rdfs:subClassOf rdf:resource="&fibo-be-oac-cctl;OverFiftyPercentControlingInterestCompany"/>
      <rdfs:subClassOf rdf:resource="&fibo-be-oac-cpty;TotalOwner"/>
   </owl:Class>

   <owl:Class rdf:about="&fibo-be-oac-cctl;VotingShareholder">
      <rdfs:label>voting shareholder</rdfs:label>
      <skos:definition>A party owning voting shares in some company limited by the issue of shares.</skos:definition>
      <rdfs:subClassOf rdf:resource="&fibo-be-oac-cown;Shareholder"/>
      <rdfs:subClassOf rdf:resource="&fibo-be-oac-cpty;DeJureControllingInterestParty"/>
   </owl:Class>

   <owl:Class rdf:about="&fibo-be-oac-cctl;VotingShareholding">
      <rdfs:label>voting shareholding</rdfs:label>
      <skos:definition>The holding of some Voting Share.</skos:definition>
      <rdfs:subClassOf rdf:resource="&fibo-be-oac-cown;Shareholding"/>
   </owl:Class>

   <owl:Class rdf:about="&fibo-be-oac-cctl;VotingShareholdingCompany">
      <rdfs:label>voting shareholding company</rdfs:label>
      <skos:definition>A Formal Business Organization which holds voting shares in some Incorporated Company.</skos:definition>
      <rdfs:subClassOf rdf:resource="&fibo-be-oac-cctl;VotingShareholder"/>
   </owl:Class>

   <owl:Class rdf:about="&fibo-be-oac-cctl;WhollyOwnedSubsidiary">
      <rdfs:label>wholly owned subsidiary</rdfs:label>
   </owl:Class>


  <!--
    ///////////////////////////////////////////////////////////////////////////////////////
    //
    // Individuals
    //
    ///////////////////////////////////////////////////////////////////////////////////////
    -->


</rdf:RDF>