<?xml version="1.0" encoding="UTF-8"?>
<!DOCTYPE rdf:RDF [
	<!ENTITY dct "http://purl.org/dc/terms/">
	<!ENTITY fibo-fnd-dt-fd "https://spec.edmcouncil.org/fibo/ontology/FND/DatesAndTimes/FinancialDates/">
	<!ENTITY fibo-fnd-rel-rel "https://spec.edmcouncil.org/fibo/ontology/FND/Relations/Relations/">
	<!ENTITY fibo-fnd-utl-alx "https://spec.edmcouncil.org/fibo/ontology/FND/Utilities/Analytics/">
	<!ENTITY fibo-fnd-utl-av "https://spec.edmcouncil.org/fibo/ontology/FND/Utilities/AnnotationVocabulary/">
	<!ENTITY owl "http://www.w3.org/2002/07/owl#">
	<!ENTITY rdf "http://www.w3.org/1999/02/22-rdf-syntax-ns#">
	<!ENTITY rdfs "http://www.w3.org/2000/01/rdf-schema#">
	<!ENTITY skos "http://www.w3.org/2004/02/skos/core#">
	<!ENTITY sm "http://www.omg.org/techprocess/ab/SpecificationMetadata/">
	<!ENTITY xsd "http://www.w3.org/2001/XMLSchema#">
]>
<rdf:RDF xml:base="https://spec.edmcouncil.org/fibo/ontology/FND/Utilities/Analytics/"
	xmlns:dct="http://purl.org/dc/terms/"
	xmlns:fibo-fnd-dt-fd="https://spec.edmcouncil.org/fibo/ontology/FND/DatesAndTimes/FinancialDates/"
	xmlns:fibo-fnd-rel-rel="https://spec.edmcouncil.org/fibo/ontology/FND/Relations/Relations/"
	xmlns:fibo-fnd-utl-alx="https://spec.edmcouncil.org/fibo/ontology/FND/Utilities/Analytics/"
	xmlns:fibo-fnd-utl-av="https://spec.edmcouncil.org/fibo/ontology/FND/Utilities/AnnotationVocabulary/"
	xmlns:owl="http://www.w3.org/2002/07/owl#"
	xmlns:rdf="http://www.w3.org/1999/02/22-rdf-syntax-ns#"
	xmlns:rdfs="http://www.w3.org/2000/01/rdf-schema#"
	xmlns:skos="http://www.w3.org/2004/02/skos/core#"
	xmlns:sm="http://www.omg.org/techprocess/ab/SpecificationMetadata/"
	xmlns:xsd="http://www.w3.org/2001/XMLSchema#">
	
	<owl:Ontology rdf:about="https://spec.edmcouncil.org/fibo/ontology/FND/Utilities/Analytics/">
		<rdfs:label>Analytics Ontology</rdfs:label>
		<dct:abstract>This ontology provides mathematical abstractions for use in other ontologies, including for example the basic components of formulae, parameters and values.</dct:abstract>
		<dct:license rdf:datatype="&xsd;anyURI">http://opensource.org/licenses/MIT</dct:license>
		<sm:contentLanguage rdf:datatype="&xsd;anyURI">http://www.w3.org/standards/techs/owl#w3c_all</sm:contentLanguage>
		<sm:copyright>Copyright (c) 2013-2019 EDM Council, Inc.</sm:copyright>
		<sm:copyright>Copyright (c) 2013-2019 Object Management Group, Inc.</sm:copyright>
		<sm:dependsOn rdf:datatype="&xsd;anyURI">https://spec.edmcouncil.org/fibo/ontology/FND/DatesAndTimes/FinancialDates/</sm:dependsOn>
		<sm:dependsOn rdf:datatype="&xsd;anyURI">https://spec.edmcouncil.org/fibo/ontology/FND/Relations/Relations/</sm:dependsOn>
		<sm:dependsOn rdf:datatype="&xsd;anyURI">https://spec.edmcouncil.org/fibo/ontology/FND/Utilities/AnnotationVocabulary/</sm:dependsOn>
		<sm:fileAbbreviation>fibo-fnd-utl-alx</sm:fileAbbreviation>
		<sm:filename>Analytics.rdf</sm:filename>
		<owl:imports rdf:resource="https://spec.edmcouncil.org/fibo/ontology/FND/DatesAndTimes/FinancialDates/"/>
		<owl:imports rdf:resource="https://spec.edmcouncil.org/fibo/ontology/FND/Relations/Relations/"/>
		<owl:imports rdf:resource="https://spec.edmcouncil.org/fibo/ontology/FND/Utilities/AnnotationVocabulary/"/>
		<owl:versionIRI rdf:resource="https://spec.edmcouncil.org/fibo/ontology/FND/20190401/Utilities/Analytics/"/>
		<skos:changeNote>The https://spec.edmcouncil.org/fibo/ontology/FND/20140501/Utilities/Analytics.rdf version of this ontology was modified per the issue resolutions identified in the FIBO FND 1.0 FTF report and in https://spec.edmcouncil.org/fibo/ontology/FND/1.0/AboutFND-1.0/.</skos:changeNote>
		<skos:changeNote>The https://spec.edmcouncil.org/fibo/ontology/FND/20141101/Utilities/Analytics.rdf version of this ontology was modified to address issue FIBOFND11-20, which added the definition of Calculation and corrected a reasoning issue related to the use of a custom datatype.</skos:changeNote>
		<skos:changeNote>The https://spec.edmcouncil.org/fibo/ontology/FND/20160201/Utilities/Analytics.rdf version of this ontology was modified per the FIBO 2.0 RFC.</skos:changeNote>
		<skos:changeNote>The https://spec.edmcouncil.org/fibo/ontology/FND/20180801/Utilities/Analytics.rdf version of this ontology was modified to use the CombinedDateTime datatype for greater flexibility in analytics.</skos:changeNote>
		<skos:changeNote>This ontology was added to Foundations in advance of the June 2014 Boston meeting in support of the IND RFC.</skos:changeNote>
		<fibo-fnd-utl-av:hasMaturityLevel rdf:resource="&fibo-fnd-utl-av;Release"/>
	</owl:Ontology>
	
	<owl:Class rdf:about="&fibo-fnd-utl-alx;CalculationFormula">
		<rdfs:subClassOf rdf:resource="&fibo-fnd-utl-alx;Formula"/>
		<rdfs:label>calculation formula</rdfs:label>
		<skos:definition>a mathematical formula that transforms one or more inputs into an amount or number of something</skos:definition>
		<fibo-fnd-utl-av:adaptedFrom rdf:datatype="&xsd;anyURI">http://www.oxforddictionaries.com/definition/english/calculation</fibo-fnd-utl-av:adaptedFrom>
		<fibo-fnd-utl-av:adaptedFrom rdf:datatype="&xsd;anyURI">https://en.wikipedia.org/wiki/Calculation</fibo-fnd-utl-av:adaptedFrom>
	</owl:Class>
	
	<owl:Class rdf:about="&fibo-fnd-utl-alx;Constant">
		<rdfs:subClassOf rdf:resource="&fibo-fnd-rel-rel;Reference"/>
		<rdfs:label>constant</rdfs:label>
		<skos:definition>a symbol that represents a constant in a formula or expression</skos:definition>
	</owl:Class>
	
	<owl:Class rdf:about="&fibo-fnd-utl-alx;Expression">
		<rdfs:subClassOf rdf:resource="&fibo-fnd-rel-rel;Reference"/>
		<rdfs:subClassOf>
			<owl:Restriction>
				<owl:onProperty rdf:resource="&fibo-fnd-utl-alx;hasArgument"/>
				<owl:onClass rdf:resource="&fibo-fnd-utl-alx;Constant"/>
				<owl:minQualifiedCardinality rdf:datatype="&xsd;nonNegativeInteger">0</owl:minQualifiedCardinality>
			</owl:Restriction>
		</rdfs:subClassOf>
		<rdfs:subClassOf>
			<owl:Restriction>
				<owl:onProperty rdf:resource="&fibo-fnd-utl-alx;hasArgument"/>
				<owl:onClass rdf:resource="&fibo-fnd-utl-alx;Variable"/>
				<owl:minQualifiedCardinality rdf:datatype="&xsd;nonNegativeInteger">0</owl:minQualifiedCardinality>
			</owl:Restriction>
		</rdfs:subClassOf>
		<rdfs:label>expression</rdfs:label>
		<skos:definition>a finite combination of symbols that are well-formed according to applicable rules</skos:definition>
	</owl:Class>
	
	<owl:Class rdf:about="&fibo-fnd-utl-alx;Formula">
		<rdfs:subClassOf rdf:resource="&fibo-fnd-rel-rel;Reference"/>
		<rdfs:subClassOf>
			<owl:Restriction>
				<owl:onProperty rdf:resource="&fibo-fnd-utl-alx;hasExpression"/>
				<owl:someValuesFrom rdf:resource="&fibo-fnd-utl-alx;Expression"/>
			</owl:Restriction>
		</rdfs:subClassOf>
		<rdfs:label>formula</rdfs:label>
		<skos:definition>a general fact or rule expressed in letters and symbols; may consist of one or more expressions</skos:definition>
		<fibo-fnd-utl-av:adaptedFrom rdf:datatype="&xsd;anyURI">http://www.merriam-webster.com/dictionary/formula</fibo-fnd-utl-av:adaptedFrom>
	</owl:Class>
	
	<owl:Class rdf:about="&fibo-fnd-utl-alx;Measure">
		<rdfs:subClassOf rdf:resource="&fibo-fnd-rel-rel;Reference"/>
		<rdfs:label>measure</rdfs:label>
		<skos:definition>an amount or degree of something; the dimensions, capacity, or amount of something ascertained by measuring</skos:definition>
		<fibo-fnd-utl-av:adaptedFrom rdf:datatype="&xsd;anyURI">http://www.merriam-webster.com/dictionary/measure</fibo-fnd-utl-av:adaptedFrom>
	</owl:Class>
	
	<owl:Class rdf:about="&fibo-fnd-utl-alx;StatisticalMeasure">
		<rdfs:subClassOf rdf:resource="&fibo-fnd-utl-alx;Measure"/>
		<rdfs:label>statistical measure</rdfs:label>
		<skos:definition>A summary (means, mode, total, index, etc.) of the individual quantitative variable values for the statistical units in a specific group (study domains).</skos:definition>
		<fibo-fnd-utl-av:definitionOrigin rdf:datatype="&xsd;anyURI">http://stats.oecd.org/glossary/detail.asp?ID=5068</fibo-fnd-utl-av:definitionOrigin>
	</owl:Class>
	
	<owl:Class rdf:about="&fibo-fnd-utl-alx;Variable">
		<rdfs:subClassOf rdf:resource="&fibo-fnd-rel-rel;Reference"/>
		<rdfs:label>variable</rdfs:label>
		<skos:definition>a symbol that represents a parameter in a formula or expression</skos:definition>
	</owl:Class>
	
	<owl:ObjectProperty rdf:about="&fibo-fnd-utl-alx;forYear">
		<rdfs:label>for calendar year</rdfs:label>
		<rdfs:domain rdf:resource="&fibo-fnd-utl-alx;StatisticalMeasure"/>
		<rdfs:range rdf:resource="&fibo-fnd-dt-fd;ExplicitDatePeriod"/>
		<skos:definition>a predicate indicating the calendar year for which the statistical measure is applicable</skos:definition>
	</owl:ObjectProperty>
	
	<owl:ObjectProperty rdf:about="&fibo-fnd-utl-alx;hasApplicableDatePeriod">
		<rdfs:subPropertyOf rdf:resource="&fibo-fnd-dt-fd;hasDatePeriod"/>
		<rdfs:label>has applicable date period</rdfs:label>
		<rdfs:domain rdf:resource="&fibo-fnd-utl-alx;StatisticalMeasure"/>
		<rdfs:range rdf:resource="&fibo-fnd-dt-fd;DatePeriod"/>
		<skos:definition>a predicate indicating the date period for which the statistical measure is applicable</skos:definition>
	</owl:ObjectProperty>
	
	<owl:DatatypeProperty rdf:about="&fibo-fnd-utl-alx;hasApplicablePeriodEnd">
		<rdfs:label>has applicable period end</rdfs:label>
		<rdfs:domain rdf:resource="&fibo-fnd-utl-alx;StatisticalMeasure"/>
		<rdfs:range rdf:resource="&fibo-fnd-dt-fd;CombinedDateTime"/>
		<skos:definition>a predicate indicating the end of the period for which the statistical measure is applicable</skos:definition>
	</owl:DatatypeProperty>
	
	<owl:DatatypeProperty rdf:about="&fibo-fnd-utl-alx;hasApplicablePeriodStart">
		<rdfs:label>has applicable period start</rdfs:label>
		<rdfs:domain rdf:resource="&fibo-fnd-utl-alx;StatisticalMeasure"/>
		<rdfs:range rdf:resource="&fibo-fnd-dt-fd;CombinedDateTime"/>
		<skos:definition>a predicate indicating the start of the period for which the statistical measure is applicable</skos:definition>
	</owl:DatatypeProperty>
	
	<owl:ObjectProperty rdf:about="&fibo-fnd-utl-alx;hasArgument">
		<rdfs:subPropertyOf rdf:resource="&fibo-fnd-rel-rel;has"/>
		<rdfs:label>has argument</rdfs:label>
		<rdfs:domain rdf:resource="&fibo-fnd-rel-rel;Reference"/>
		<rdfs:range rdf:resource="&fibo-fnd-rel-rel;Reference"/>
		<skos:definition>indicates a specific input to a function, formula or expression, also known as an independent variable</skos:definition>
	</owl:ObjectProperty>
	
	<owl:ObjectProperty rdf:about="&fibo-fnd-utl-alx;hasExpression">
		<rdfs:subPropertyOf rdf:resource="&fibo-fnd-rel-rel;has"/>
		<rdfs:label>has expression</rdfs:label>
		<rdfs:domain rdf:resource="&fibo-fnd-rel-rel;Reference"/>
		<rdfs:range rdf:resource="&fibo-fnd-utl-alx;Expression"/>
		<skos:definition>indicates a mathematical or other formal expression, which may be part of a formula</skos:definition>
	</owl:ObjectProperty>
	
	<owl:ObjectProperty rdf:about="&fibo-fnd-utl-alx;hasFormula">
		<rdfs:subPropertyOf rdf:resource="&fibo-fnd-rel-rel;has"/>
		<rdfs:label>has formula</rdfs:label>
		<rdfs:range rdf:resource="&fibo-fnd-utl-alx;Formula"/>
		<skos:definition>indicates a concise way of expressing information symbolically, as in a mathematical or chemical formula</skos:definition>
	</owl:ObjectProperty>
	
	<owl:DatatypeProperty rdf:about="&fibo-fnd-utl-alx;hasMeasurementDate">
		<rdfs:subPropertyOf rdf:resource="&fibo-fnd-dt-fd;hasDateValue"/>
		<rdfs:label>has measurement date</rdfs:label>
		<rdfs:domain rdf:resource="&fibo-fnd-utl-alx;Measure"/>
		<rdfs:range rdf:resource="&fibo-fnd-dt-fd;dateValue"/>
		<skos:definition>a predicate indicating the date on which the measure was taken</skos:definition>
	</owl:DatatypeProperty>
	
	<owl:DatatypeProperty rdf:about="&fibo-fnd-utl-alx;hasMeasurementPeriodInMonths">
		<rdfs:label>has measurement period in months</rdfs:label>
		<rdfs:domain rdf:resource="&fibo-fnd-utl-alx;Measure"/>
		<rdfs:range rdf:resource="&xsd;integer"/>
		<skos:definition>a predicate indicating the coverage period for which the measure is applicable expressed in months</skos:definition>
	</owl:DatatypeProperty>
	
	<owl:DatatypeProperty rdf:about="&fibo-fnd-utl-alx;hasNumberOfEntries">
		<rdfs:subPropertyOf rdf:resource="&fibo-fnd-dt-fd;hasCount"/>
		<rdfs:label>has number of entries</rdfs:label>
		<rdfs:range rdf:resource="&xsd;positiveInteger"/>
		<skos:definition>a predicate indicated the number of elements in some document, table, or other resource (e.g., in a report, table)</skos:definition>
	</owl:DatatypeProperty>
	
	<owl:ObjectProperty rdf:about="&fibo-fnd-utl-alx;hasOperand">
		<rdfs:subPropertyOf rdf:resource="&fibo-fnd-rel-rel;has"/>
		<rdfs:label>has operand</rdfs:label>
		<rdfs:domain rdf:resource="&fibo-fnd-rel-rel;Reference"/>
		<rdfs:range rdf:resource="&fibo-fnd-rel-rel;Referent"/>
		<skos:definition>indicates the operand of a mathematical argument, parameter or other similar concept</skos:definition>
	</owl:ObjectProperty>
	
	<owl:ObjectProperty rdf:about="&fibo-fnd-utl-alx;isMeasureOf">
		<rdfs:subPropertyOf rdf:resource="&fibo-fnd-rel-rel;appliesTo"/>
		<rdfs:label>is a measure of</rdfs:label>
		<rdfs:domain rdf:resource="&fibo-fnd-utl-alx;Measure"/>
		<skos:definition>a predicate indicating the concept being measured</skos:definition>
	</owl:ObjectProperty>

</rdf:RDF>