<?xml version="1.0" encoding="UTF-8"?>
<!DOCTYPE rdf:RDF [
	<!ENTITY dct "http://purl.org/dc/terms/">
	<!ENTITY fibo-fnd-utl-av "https://spec.edmcouncil.org/fibo/ontology/FND/Utilities/AnnotationVocabulary/">
	<!ENTITY owl "http://www.w3.org/2002/07/owl#">
	<!ENTITY rdf "http://www.w3.org/1999/02/22-rdf-syntax-ns#">
	<!ENTITY rdfs "http://www.w3.org/2000/01/rdf-schema#">
	<!ENTITY skos "http://www.w3.org/2004/02/skos/core#">
	<!ENTITY sm "http://www.omg.org/techprocess/ab/SpecificationMetadata/">
	<!ENTITY xsd "http://www.w3.org/2001/XMLSchema#">
]>
<rdf:RDF xml:base="https://spec.edmcouncil.org/fibo/ontology/FND/Utilities/AnnotationVocabulary/"
	xmlns:dct="http://purl.org/dc/terms/"
	xmlns:fibo-fnd-utl-av="https://spec.edmcouncil.org/fibo/ontology/FND/Utilities/AnnotationVocabulary/"
	xmlns:owl="http://www.w3.org/2002/07/owl#"
	xmlns:rdf="http://www.w3.org/1999/02/22-rdf-syntax-ns#"
	xmlns:rdfs="http://www.w3.org/2000/01/rdf-schema#"
	xmlns:skos="http://www.w3.org/2004/02/skos/core#"
	xmlns:sm="http://www.omg.org/techprocess/ab/SpecificationMetadata/"
	xmlns:xsd="http://www.w3.org/2001/XMLSchema#">
	
	<owl:Ontology rdf:about="https://spec.edmcouncil.org/fibo/ontology/FND/Utilities/AnnotationVocabulary/">
		<rdfs:label>Annotation Vocabulary</rdfs:label>
		<dct:abstract>This vocabulary provides a set of metadata annotations for use in describing FIBO ontology elements.  The annotations extend properties defined in the OMG&apos;s Specification Metadata Recommendation, in the Dublin Core Metadata Terms Vocabulary and in the W3C Simple Knowledge Organization System (SKOS) Vocabulary, and have been customized to suit the FIBO specification development process.  

Note that any of the original properties provided in Dublin Core and SKOS can be used in addition to the terms provided herein.  However, any Dublin Core terms that are not explicitly defined as OWL annotation properties in this ontology or in any of its imports must be so declared in the ontologies that use them.</dct:abstract>
		<dct:license rdf:datatype="&xsd;anyURI">http://opensource.org/licenses/MIT</dct:license>
		<sm:contentLanguage rdf:datatype="&xsd;anyURI">http://www.w3.org/standards/techs/owl#w3c_all</sm:contentLanguage>
		<sm:copyright>Copyright (c) 2013-2020 EDM Council, Inc.</sm:copyright>
		<sm:copyright>Copyright (c) 2013-2020 Object Management Group, Inc.</sm:copyright>
		<sm:fileAbbreviation>fibo-fnd-utl-av</sm:fileAbbreviation>
		<sm:filename>AnnotationVocabulary.rdf</sm:filename>
		<owl:imports rdf:resource="http://www.omg.org/techprocess/ab/SpecificationMetadata/"/>
		<owl:imports rdf:resource="http://www.w3.org/2004/02/skos/core"/>
		<owl:versionIRI rdf:resource="https://spec.edmcouncil.org/fibo/ontology/FND/20200301/Utilities/AnnotationVocabulary/"/>
		<skos:changeNote>The http://www.omg.org/spec/EDMC-FIBO/FND/20130801/Utilities/AnnotationVocabulary.rdf version of this ontology was modified per the issue resolutions identified in the FIBO FND 1.0 FTF report and in http://www.omg.org/spec/EDMC-FIBO/FND/1.0/AboutFND-1.0/.</skos:changeNote>
		<skos:changeNote>The http://www.omg.org/spec/FIBO/Foundations/20130601/Utilities/AnnotationVocabulary.owl version of the ontology was revised in advance of the September 2013 New Brunswick, NJ meeting, as follows:
   (1) to use slash style URI/IRIss (also called 303 URIs, vs. hash style) as required to support server side processing 
   (2) to use version-independent IRIs for all definitions internally as opposed to version-specific IRIs
   (3) to change the file suffix from .owl to .rdf to increase usability in RDF tools
   (4) to use 4-level abbreviations and corresponding namespace prefixes for all FIBO ontologies, reflecting a family/specification/module/ontology structure
   (5) to incorporate changes to the specification metadata to support documentation at the family, specification, module, and ontology level, similar to the abbreviations</skos:changeNote>
		<skos:changeNote>The https://spec.edmcouncil.org/fibo/ontology/FND/20180801/Utilities/AnnotationVocabulary.rdf version of this ontology was modified to add the symbol annotation.</skos:changeNote>
		<skos:changeNote>The https://spec.edmcouncil.org/fibo/ontology/FND/20190501/Utilities/AnnotationVocabulary.rdf version of this ontology was modified to eliminate deprecated properties.</skos:changeNote>
		<skos:changeNote>The https://spec.edmcouncil.org/fibo/ontology/FND/20190901/Utilities/AnnotationVocabulary.rdf version of this ontology was modified to add common and preferred designations as needed for postal addresses and other purposes, to correct named individuals to be properly declared, and to revise definitions to be ISO 704 compliant.</skos:changeNote>
		<fibo-fnd-utl-av:hasMaturityLevel rdf:resource="&fibo-fnd-utl-av;Release"/>
	</owl:Ontology>
	
	<owl:AnnotationProperty rdf:about="&dct;modified">
	</owl:AnnotationProperty>
	
	<owl:NamedIndividual rdf:about="&fibo-fnd-utl-av;Informative">
		<rdf:type rdf:resource="&fibo-fnd-utl-av;MaturityLevel"/>
		<rdfs:label>informative</rdfs:label>
		<skos:definition xml:lang="en">entity that is considered deprecated but included for informational purposes because it is referenced by some provisional concept</skos:definition>
		<fibo-fnd-utl-av:explanatoryNote xml:lang="en">Informative content will be removed as soon as all dependencies have been eliminated, thus FIBO users should not depend on it going forward.</fibo-fnd-utl-av:explanatoryNote>
	</owl:NamedIndividual>
	
	<owl:Class rdf:about="&fibo-fnd-utl-av;MaturityLevel">
		<rdfs:subClassOf rdf:resource="&skos;Concept"/>
		<rdfs:label>maturity level</rdfs:label>
		<skos:definition>classifier used to indicate state of an artifact with respect to its development lifecycle</skos:definition>
		<fibo-fnd-utl-av:explanatoryNote xml:lang="en">FIBO currently has three maturity levels: Informative, Provisional, and Release.</fibo-fnd-utl-av:explanatoryNote>
	</owl:Class>
	
	<owl:NamedIndividual rdf:about="&fibo-fnd-utl-av;Provisional">
		<rdf:type rdf:resource="&fibo-fnd-utl-av;MaturityLevel"/>
		<rdfs:label>provisional</rdfs:label>
		<skos:definition xml:lang="en">entity that is considered to be under development</skos:definition>
		<fibo-fnd-utl-av:explanatoryNote xml:lang="en">Provisional content is subject to change, and may change substantially prior to release. FIBO users should be aware that it is not dependable, but could be used for informative reference and as the basis for further work.  Release notes with respect to provisional content are likely to be sketchy at best, and users should not expect official change notes to mention it.</fibo-fnd-utl-av:explanatoryNote>
	</owl:NamedIndividual>
	
	<owl:NamedIndividual rdf:about="&fibo-fnd-utl-av;Release">
		<rdf:type rdf:resource="&fibo-fnd-utl-av;MaturityLevel"/>
		<rdfs:label>release</rdfs:label>
		<skos:definition xml:lang="en">entity that is considered to be stable and mature from a development perspective</skos:definition>
		<fibo-fnd-utl-av:explanatoryNote xml:lang="en">Release notes will be provided for any changes with respect to released content, and any revisions will be backwards compatible with the prior version to the degree possible.</fibo-fnd-utl-av:explanatoryNote>
	</owl:NamedIndividual>
	
	<owl:AnnotationProperty rdf:about="&fibo-fnd-utl-av;abbreviation">
		<rdfs:subPropertyOf rdf:resource="&skos;altLabel"/>
		<rdfs:label>abbreviation</rdfs:label>
		<skos:definition>short form designation for an entity that can be substituted for its primary representation</skos:definition>
		<fibo-fnd-utl-av:adaptedFrom>ISO 1087-1 Terminology work - Vocabulary</fibo-fnd-utl-av:adaptedFrom>
	</owl:AnnotationProperty>
	
	<owl:AnnotationProperty rdf:about="&fibo-fnd-utl-av;adaptedFrom">
		<rdfs:subPropertyOf rdf:resource="&sm;directSource"/>
		<rdfs:label>adapted from</rdfs:label>
		<skos:definition>document or other source from which a given term (or its definition) was adapted; the range for this annotation can be a string, URI, or BibliographicCitation</skos:definition>
	</owl:AnnotationProperty>
	
	<owl:AnnotationProperty rdf:about="&fibo-fnd-utl-av;commonDesignation">
		<rdfs:subPropertyOf rdf:resource="&skos;altLabel"/>
		<rdfs:label>common designation</rdfs:label>
		<skos:definition>frequently used designation for an entity</skos:definition>
		<fibo-fnd-utl-av:adaptedFrom rdf:datatype="&xsd;anyURI">https://pe.usps.com/cpim/ftp/pubs/Pub28/pub28.pdf</fibo-fnd-utl-av:adaptedFrom>
	</owl:AnnotationProperty>
	
	<owl:AnnotationProperty rdf:about="&fibo-fnd-utl-av;definitionOrigin">
		<rdfs:subPropertyOf rdf:resource="&sm;directSource"/>
		<rdfs:label>definition origin</rdfs:label>
		<skos:definition>document or other source from which a given definition was taken directly; the range for this annotation can be a string, URI, or BibliographicCitation</skos:definition>
	</owl:AnnotationProperty>
	
	<owl:AnnotationProperty rdf:about="&fibo-fnd-utl-av;explanatoryNote">
		<rdfs:subPropertyOf rdf:resource="&skos;note"/>
		<rdfs:label>explanatory note</rdfs:label>
		<skos:definition>note that provides additional explanatory information about a given concept</skos:definition>
	</owl:AnnotationProperty>
	
	<owl:AnnotationProperty rdf:about="&fibo-fnd-utl-av;hasMaturityLevel">
		<rdfs:label>has maturity level</rdfs:label>
		<skos:definition>links something to its state with respect to a development lifecycle</skos:definition>
	</owl:AnnotationProperty>
	
	<owl:AnnotationProperty rdf:about="&fibo-fnd-utl-av;logicalDefinition">
		<rdfs:label>logical definition</rdfs:label>
		<skos:definition>description of the OWL logic of a model element in natural language</skos:definition>
	</owl:AnnotationProperty>
	
	<owl:AnnotationProperty rdf:about="&fibo-fnd-utl-av;modifiedBy">
		<rdfs:subPropertyOf rdf:resource="&sm;contributor"/>
		<rdfs:label>modified by</rdfs:label>
		<skos:definition>organization or person responsible for making a change to a model element</skos:definition>
	</owl:AnnotationProperty>
	
	<owl:AnnotationProperty rdf:about="&fibo-fnd-utl-av;modifiedOn">
		<rdfs:subPropertyOf rdf:resource="&dct;modified"/>
		<rdfs:label>modified on</rdfs:label>
		<skos:definition>date a model element was changed</skos:definition>
	</owl:AnnotationProperty>
	
	<owl:AnnotationProperty rdf:about="&fibo-fnd-utl-av;preferredDesignation">
		<rdfs:subPropertyOf rdf:resource="&skos;altLabel"/>
		<rdfs:label>preferred designation</rdfs:label>
		<skos:definition>recommended designation for an entity in some context</skos:definition>
		<fibo-fnd-utl-av:adaptedFrom rdf:datatype="&xsd;anyURI">https://pe.usps.com/cpim/ftp/pubs/Pub28/pub28.pdf</fibo-fnd-utl-av:adaptedFrom>
	</owl:AnnotationProperty>
	
	<owl:AnnotationProperty rdf:about="&fibo-fnd-utl-av;symbol">
		<rdfs:subPropertyOf rdf:resource="&fibo-fnd-utl-av;abbreviation"/>
		<rdfs:label>symbol</rdfs:label>
		<skos:definition>abbreviation that is a design, mark, or character(s) used conventionally to represent something, such as a currency, quantity, or variable in an expression</skos:definition>
		<fibo-fnd-utl-av:adaptedFrom>ISO 31-0 Quantities and units - General principles</fibo-fnd-utl-av:adaptedFrom>
		<fibo-fnd-utl-av:explanatoryNote>The symbols for quantities are generally single letters of the Latin or Greek alphabet, sometimes with subscripts or other modifying signs.</fibo-fnd-utl-av:explanatoryNote>
	</owl:AnnotationProperty>
	
	<owl:AnnotationProperty rdf:about="&fibo-fnd-utl-av;synonym">
		<rdfs:subPropertyOf rdf:resource="&skos;altLabel"/>
		<rdfs:label>synonym</rdfs:label>
		<skos:definition>designation that can be substituted for the primary representation of something</skos:definition>
		<fibo-fnd-utl-av:adaptedFrom>ISO 1087-1 Terminology work - Vocabulary</fibo-fnd-utl-av:adaptedFrom>
	</owl:AnnotationProperty>
	
	<owl:AnnotationProperty rdf:about="&fibo-fnd-utl-av;termOrigin">
		<rdfs:subPropertyOf rdf:resource="&sm;directSource"/>
		<rdfs:label>term origin</rdfs:label>
		<skos:definition>document or other source from which a given term was taken directly; the range for this annotation can be a string, URI, or BibliographicCitation</skos:definition>
	</owl:AnnotationProperty>
	
	<owl:AnnotationProperty rdf:about="&fibo-fnd-utl-av;usageNote">
		<rdfs:subPropertyOf rdf:resource="&skos;note"/>
		<rdfs:label>usage note</rdfs:label>
		<skos:definition>note that provides information about how a given concept should be used or extended</skos:definition>
	</owl:AnnotationProperty>

</rdf:RDF>