<?xml version="1.0" encoding="UTF-8"?>
<rdf:RDF xmlns:xsd="http://www.w3.org/2001/XMLSchema#"
         xmlns:sm="http://www.omg.org/techprocess/ab/SpecificationMetadata/"
         xmlns:fibo-fnd-utl-av="http://www.omg.org/spec/EDMC-FIBO/FND/Utilities/AnnotationVocabulary/"
         xmlns:rdf="http://www.w3.org/1999/02/22-rdf-syntax-ns#"
         xmlns:rdfs="http://www.w3.org/2000/01/rdf-schema#"
         xmlns:owl="http://www.w3.org/2002/07/owl#"
         xmlns:skos="http://www.w3.org/2004/02/skos/core#"
         xmlns:dc="http://purl.org/dc/terms/"
         xml:base="http://www.edmcouncil.org/spec/EDMC-SR/BE/CorporationsExt/CorporationEquity/">

   <owl:Ontology rdf:about="http://www.edmcouncil.org/spec/EDMC-SR/BE/CorporationsExt/CorporationEquity/">
      <owl:imports rdf:resource="http://www.omg.org/spec/EDMC-SR/BE/Corporations/Corporations/"/>
      <owl:imports rdf:resource="http://www.omg.org/spec/EDMC-FIBO/SEC/Equities/EquityInstruments/"/>
      <owl:imports rdf:resource="http://www.omg.org/spec/EDMC-SR/BE/OwnershipAndControl/CorporateOwnership/"/>
   </owl:Ontology>

   <!--Datatypes-->

<!--Object Properties-->

<owl:ObjectProperty rdf:about="http://www.edmcouncil.org/spec/EDMC-SR/BE/CorporationsExt/CorporationEquity/owns">
      <skos:definition>Publicly issued equity in a company incorporated by shares, owned by the business entity.</skos:definition>
      <rdfs:subPropertyOf rdf:resource="http://www.edmcouncil.org/spec/EDMC-SR/BE/CorporationsExt/CorporationEquity/owns.1"/>
      <rdfs:domain rdf:resource="http://www.omg.org/spec/EDMC-SR/BE/LegalEntities/FormalBusinessOrganizations/FormallyConstitutedOrganization"/>
      <rdfs:range rdf:resource="http://www.omg.org/spec/EDMC-FIBO/SEC/Equities/EquityInstruments/PubliclyIssuedEquity"/>
   </owl:ObjectProperty>

   <owl:ObjectProperty rdf:about="http://www.edmcouncil.org/spec/EDMC-SR/BE/CorporationsExt/CorporationEquity/owns.1">
      <skos:definition>Equity in a company incorporated by shares, owned privately or publicly by the business entity.</skos:definition>
      <rdfs:domain rdf:resource="http://www.omg.org/spec/EDMC-SR/BE/LegalEntities/FormalBusinessOrganizations/FormallyConstitutedOrganization"/>
      <rdfs:range rdf:resource="http://www.omg.org/spec/EDMC-SR/FND/Accounting/AccountingEquity/StockholdersEquity"/>
   </owl:ObjectProperty>

   <owl:ObjectProperty rdf:about="http://www.edmcouncil.org/spec/EDMC-SR/BE/CorporationsExt/CorporationEquity/governingLaw">
      <skos:definition>The Jurisdiction in which the Company Legal Form is defined.</skos:definition>
      <rdfs:domain rdf:resource="http://www.omg.org/spec/EDMC-SR/BE/OwnershipAndControl/Executives/ArticlesOfIncorporation"/>
      <rdfs:range rdf:resource="http://www.omg.org/spec/EDMC-SR/FND/Law/Jurisdictions/Jurisdiction"/>
   </owl:ObjectProperty>

   <owl:ObjectProperty rdf:about="http://www.edmcouncil.org/spec/EDMC-SR/BE/CorporationsExt/CorporationEquity/governedBy">
      <skos:definition>The Company constitution or Articles of Inforporation, Articles of Association etc. which defines the terms for equity instruments issued by that company.</skos:definition>
      <rdfs:domain rdf:resource="http://www.omg.org/spec/EDMC-FIBO/SEC/Equities/EquityInstruments/Share"/>
      <rdfs:range rdf:resource="http://www.omg.org/spec/EDMC-SR/BE/OwnershipAndControl/Executives/ArticlesOfIncorporation"/>
   </owl:ObjectProperty>

   <owl:ObjectProperty rdf:about="http://www.edmcouncil.org/spec/EDMC-SR/BE/CorporationsExt/CorporationEquity/hasMajorityHoldingOfAnotherCompanys">
      <skos:definition>Majority Equity held by the company, in another company. This is assumed to be publicly issued equity.</skos:definition>
      <rdfs:subPropertyOf rdf:resource="http://www.edmcouncil.org/spec/EDMC-SR/BE/CorporationsExt/CorporationEquity/hasHoldingOfAnotherCompanys"/>
      <rdfs:domain rdf:resource="http://www.omg.org/spec/EDMC-SR/BE/Corporations/Corporations/IncorporatedCompany"/>
      <rdfs:range rdf:resource="http://www.omg.org/spec/EDMC-FIBO/SEC/Equities/EquityInstruments/PubliclyIssuedEquity"/>
   </owl:ObjectProperty>

   <owl:ObjectProperty rdf:about="http://www.edmcouncil.org/spec/EDMC-SR/BE/CorporationsExt/CorporationEquity/hasHoldingOfAnotherCompanys">
      <skos:definition>Equity held by the company, in another company. This is assumed to be publicly issued equity.</skos:definition>
      <rdfs:subPropertyOf rdf:resource="http://www.edmcouncil.org/spec/EDMC-SR/BE/CorporationsExt/CorporationEquity/owns"/>
      <rdfs:domain rdf:resource="http://www.omg.org/spec/EDMC-SR/BE/Corporations/Corporations/IncorporatedCompany"/>
      <rdfs:range rdf:resource="http://www.omg.org/spec/EDMC-FIBO/SEC/Equities/EquityInstruments/PubliclyIssuedEquity"/>
   </owl:ObjectProperty>

   <owl:ObjectProperty rdf:about="http://www.edmcouncil.org/spec/EDMC-SR/BE/CorporationsExt/CorporationEquity/hasCapital">
      <skos:definition>The capital issued by the company at its formation or subsequently.</skos:definition>
      <rdfs:subPropertyOf rdf:resource="http://www.edmcouncil.org/spec/EDMC-SR/BE/CorporationsExt/CorporationEquity/hasCapital.2"/>
      <rdfs:domain rdf:resource="http://www.omg.org/spec/EDMC-SR/BE/Corporations/Corporations/PrivatelyHeldCompany"/>
      <rdfs:range rdf:resource="http://www.omg.org/spec/EDMC-FIBO/SEC/Equities/EquityInstruments/PrivateEquity"/>
   </owl:ObjectProperty>

   <owl:ObjectProperty rdf:about="http://www.edmcouncil.org/spec/EDMC-SR/BE/CorporationsExt/CorporationEquity/hasCapital.1">
      <skos:definition>Capital issued publicly by the company and held by the public.</skos:definition>
      <rdfs:subPropertyOf rdf:resource="http://www.edmcouncil.org/spec/EDMC-SR/BE/CorporationsExt/CorporationEquity/hasCapital.2"/>
      <rdfs:domain rdf:resource="http://www.omg.org/spec/EDMC-SR/BE/Corporations/Corporations/PubliclyHeldCompany"/>
      <rdfs:range rdf:resource="http://www.omg.org/spec/EDMC-FIBO/SEC/Equities/EquityInstruments/PubliclyIssuedEquity"/>
   </owl:ObjectProperty>

   <owl:ObjectProperty rdf:about="http://www.edmcouncil.org/spec/EDMC-SR/BE/CorporationsExt/CorporationEquity/mayHaveCapitalAs">
      <skos:definition>Additional privately held equity in the company, which is not held as publicly issued shares.</skos:definition>
      <rdfs:subPropertyOf rdf:resource="http://www.edmcouncil.org/spec/EDMC-SR/BE/CorporationsExt/CorporationEquity/hasCapital.2"/>
      <rdfs:domain rdf:resource="http://www.omg.org/spec/EDMC-SR/BE/Corporations/Corporations/PubliclyHeldCompany"/>
      <rdfs:range rdf:resource="http://www.omg.org/spec/EDMC-FIBO/SEC/Equities/EquityInstruments/PrivateEquity"/>
   </owl:ObjectProperty>

   <owl:ObjectProperty rdf:about="http://www.edmcouncil.org/spec/EDMC-SR/BE/CorporationsExt/CorporationEquity/setOutIn">
      <rdfs:domain rdf:resource="http://www.omg.org/spec/EDMC-FIBO/SEC/Equities/EquityInstruments/VotingRight"/>
      <rdfs:range rdf:resource="http://www.omg.org/spec/EDMC-SR/BE/OwnershipAndControl/Executives/ArticlesOfIncorporation"/>
   </owl:ObjectProperty>

   <owl:ObjectProperty rdf:about="http://www.edmcouncil.org/spec/EDMC-SR/BE/CorporationsExt/CorporationEquity/hasCapital.2">
      <skos:definition>The capital issued by the company at its formation or subsequently.</skos:definition>
      <skos:editorialNote>Review comment: Participation is not necessarily a share. Ownership of the capital.</skos:editorialNote>
      <rdfs:subPropertyOf rdf:resource="http://www.omg.org/spec/EDMC-SR/BE/LegalEntities/CorporateBodies/issuesEquity"/>
      <rdfs:domain rdf:resource="http://www.omg.org/spec/EDMC-SR/BE/Corporations/Corporations/IncorporatedCompany"/>
      <rdfs:range rdf:resource="http://www.omg.org/spec/EDMC-FIBO/SEC/Equities/EquityInstruments/ShareholderEquity"/>
   </owl:ObjectProperty>

   <!--Data Properties-->

<!--Annotation Properties-->

<!--Classes-->

<!--Individuals-->

</rdf:RDF>