<?xml version="1.0" encoding="UTF-8"?>
<rdf:RDF xmlns:xsd="http://www.w3.org/2001/XMLSchema#"
         xmlns:sm="http://www.omg.org/techprocess/ab/SpecificationMetadata/"
         xmlns:fibo-fnd-utl-av="http://www.omg.org/spec/EDMC-FIBO/FND/Utilities/AnnotationVocabulary/"
         xmlns:rdf="http://www.w3.org/1999/02/22-rdf-syntax-ns#"
         xmlns:rdfs="http://www.w3.org/2000/01/rdf-schema#"
         xmlns:owl="http://www.w3.org/2002/07/owl#"
         xmlns:skos="http://www.w3.org/2004/02/skos/core#"
         xmlns:dc="http://purl.org/dc/terms/"
         xml:base="http://www.omg.org/spec/EDMC-SR/BE/OwnershipAndControl/Executives/">

   <owl:Ontology rdf:about="http://www.omg.org/spec/EDMC-SR/BE/OwnershipAndControl/Executives/">
      <owl:imports rdf:resource="http://www.omg.org/spec/EDMC-SR/BE/OwnershipAndControl/ControlParties/"/>
      <owl:imports rdf:resource="http://www.omg.org/spec/EDMC-SR/FND/Law/LegalCapacities/"/>
   </owl:Ontology>

   <!--Datatypes-->

<!--Object Properties-->

<owl:ObjectProperty rdf:about="http://www.omg.org/spec/EDMC-SR/BE/OwnershipAndControl/Executives/boardCapacityIsConferredBy">
      <skos:definition>The instrument which confers the Board Capacity. This is either the Company By-laws or the Board Agreement.</skos:definition>
      <skos:editorialNote>The precise instrument by which the capacity is conferred vary from one capacity to another, i.e. some will be defined in the By-laws and others will be defined in the Board Agreement.</skos:editorialNote>
      <rdfs:subPropertyOf rdf:resource="http://www.omg.org/spec/EDMC-SR/FND/Law/LegalCapacities/isConferredBy"/>
      <rdfs:domain rdf:resource="http://www.omg.org/spec/EDMC-SR/BE/OwnershipAndControl/Executives/BoardCapacity"/>
      <rdfs:range rdf:resource="http://www.omg.org/spec/EDMC-SR/BE/OwnershipAndControl/Executives/Anon-19003"/>
   </owl:ObjectProperty>

   <owl:ObjectProperty rdf:about="http://www.omg.org/spec/EDMC-SR/BE/OwnershipAndControl/Executives/boardMemberIsAPartyTo">
      <rdfs:subPropertyOf rdf:resource="http://www.omg.org/spec/EDMC-SR/FND/Parties/Parties/isAPartyTo"/>
      <rdfs:domain rdf:resource="http://www.omg.org/spec/EDMC-SR/BE/OwnershipAndControl/Executives/BoardMember"/>
      <rdfs:range rdf:resource="http://www.omg.org/spec/EDMC-SR/BE/Corporations/Corporations/BoardAgreement"/>
   </owl:ObjectProperty>

   <owl:ObjectProperty rdf:about="http://www.omg.org/spec/EDMC-SR/BE/OwnershipAndControl/Executives/boardOfDirectorsAppoints">
      <skos:definition>The board of the company has the power to appoint the individuals who are to be the public officers of the company.</skos:definition>
      <rdfs:subPropertyOf rdf:resource="http://www.omg.org/spec/EDMC-SR/FND/Relations/Relations/appoints"/>
      <rdfs:domain rdf:resource="http://www.omg.org/spec/EDMC-SR/BE/OwnershipAndControl/Executives/BoardOfDirectors"/>
      <rdfs:range rdf:resource="http://www.omg.org/spec/EDMC-SR/BE/OwnershipAndControl/Executives/CorporateOfficer"/>
   </owl:ObjectProperty>

   <owl:ObjectProperty rdf:about="http://www.omg.org/spec/EDMC-SR/BE/OwnershipAndControl/Executives/companyBoardHasVestedInIt">
      <skos:definition>The board of a company has some legal capacity vested in it.</skos:definition>
      <rdfs:subPropertyOf rdf:resource="http://www.omg.org/spec/EDMC-SR/FND/Law/LegalCapacities/hasCapacity"/>
      <rdfs:domain rdf:resource="http://www.omg.org/spec/EDMC-SR/BE/OwnershipAndControl/Executives/BoardOfDirectors"/>
      <rdfs:range rdf:resource="http://www.omg.org/spec/EDMC-SR/BE/OwnershipAndControl/Executives/BoardCapacity"/>
   </owl:ObjectProperty>

   <owl:ObjectProperty rdf:about="http://www.omg.org/spec/EDMC-SR/BE/OwnershipAndControl/Executives/boardOfDirectorsHasIdentity">
      <rdfs:subPropertyOf rdf:resource="http://www.omg.org/spec/EDMC-SR/FND/Parties/Parties/partyInRoleHasIdentity"/>
      <rdfs:domain rdf:resource="http://www.omg.org/spec/EDMC-SR/BE/OwnershipAndControl/Executives/BoardOfDirectors"/>
      <rdfs:range rdf:resource="http://www.omg.org/spec/EDMC-SR/FND/Organizations/FormalOrganizations/Group"/>
   </owl:ObjectProperty>

   <owl:ObjectProperty rdf:about="http://www.omg.org/spec/EDMC-SR/BE/OwnershipAndControl/Executives/boardOfDirectorsHasMember">
      <skos:definition>The board has a number of members who collectively exercise the powers of that board.</skos:definition>
      <rdfs:subPropertyOf rdf:resource="http://www.omg.org/spec/EDMC-SR/FND/Relations/Relations/hasMember"/>
      <rdfs:subPropertyOf rdf:resource="http://www.edmcouncil.org/spec/EDMC-SR/FND/Relative/Collections/hasConstituent"/>
      <rdfs:domain rdf:resource="http://www.omg.org/spec/EDMC-SR/BE/OwnershipAndControl/Executives/BoardOfDirectors"/>
      <rdfs:range rdf:resource="http://www.omg.org/spec/EDMC-SR/BE/OwnershipAndControl/Executives/BoardMember"/>
   </owl:ObjectProperty>

   <owl:ObjectProperty rdf:about="http://www.omg.org/spec/EDMC-SR/BE/OwnershipAndControl/Executives/constrains">
      <skos:definition>The Instrument of Incorporation (being effectively the constitution of the entity) governs and constrains the application of the bylaws of the company.</skos:definition>
      <rdfs:subPropertyOf rdf:resource="http://www.omg.org/spec/EDMC-SR/FND/Relations/Relations/constrains"/>
      <rdfs:domain rdf:resource="http://www.omg.org/spec/EDMC-SR/BE/LegalEntities/CorporateBodies/InstrumentOfIncorporation"/>
      <rdfs:range rdf:resource="http://www.omg.org/spec/EDMC-SR/BE/OwnershipAndControl/Executives/CompanyBylaw"/>
   </owl:ObjectProperty>

   <owl:ObjectProperty rdf:about="http://www.omg.org/spec/EDMC-SR/BE/OwnershipAndControl/Executives/companyOfficerLegalCapacityConferredBy">
      <skos:definition>The capacity of the public officer is conferred by one or another ot the company legal form documentation (articles of association or equivalent) or some company by-law.</skos:definition>
      <rdfs:subPropertyOf rdf:resource="http://www.omg.org/spec/EDMC-SR/FND/Law/LegalCapacities/isConferredBy"/>
      <rdfs:domain rdf:resource="http://www.omg.org/spec/EDMC-SR/BE/OwnershipAndControl/Executives/CorporateOfficerCapacity"/>
      <rdfs:range rdf:resource="http://www.omg.org/spec/EDMC-SR/BE/OwnershipAndControl/Executives/CompanyLaw"/>
   </owl:ObjectProperty>

   <owl:ObjectProperty rdf:about="http://www.omg.org/spec/EDMC-SR/BE/OwnershipAndControl/Executives/mandatedBy">
      <skos:definition>The Statutory Obligation is mandated by some piece of Company Law.</skos:definition>
      <rdfs:subPropertyOf rdf:resource="http://www.omg.org/spec/EDMC-SR/FND/Law/LegalCapacities/statutoryResponsibilityIsMandatedBy"/>
      <rdfs:domain rdf:resource="http://www.omg.org/spec/EDMC-SR/BE/OwnershipAndControl/Executives/CompanyStatutoryObligation"/>
      <rdfs:range rdf:resource="http://www.omg.org/spec/EDMC-SR/BE/OwnershipAndControl/Executives/CompanyLaw"/>
   </owl:ObjectProperty>

   <owl:ObjectProperty rdf:about="http://www.omg.org/spec/EDMC-SR/BE/OwnershipAndControl/Executives/definedBy">
      <skos:definition>The legal capacity of the Public Officer is set out in some piee of Company Law.</skos:definition>
      <rdfs:subPropertyOf rdf:resource="http://www.omg.org/spec/EDMC-SR/FND/Relations/Relations/isGoverneBy"/>
      <rdfs:domain rdf:resource="http://www.omg.org/spec/EDMC-SR/BE/OwnershipAndControl/Executives/CorporateOfficerCapacity"/>
      <rdfs:range rdf:resource="http://www.omg.org/spec/EDMC-SR/BE/OwnershipAndControl/Executives/CompanyLaw"/>
   </owl:ObjectProperty>

   <owl:ObjectProperty rdf:about="http://www.omg.org/spec/EDMC-SR/BE/OwnershipAndControl/Executives/publicOfficerIdentity">
      <skos:definition>That which is the Public Officer. This must be a natural person and also must be an adult.</skos:definition>
      <rdfs:subPropertyOf rdf:resource="http://www.omg.org/spec/EDMC-SR/BE/OwnershipAndControl/Executives/legallyDelegatedAuthorityHasIdentity"/>
      <rdfs:domain rdf:resource="http://www.omg.org/spec/EDMC-SR/BE/OwnershipAndControl/Executives/CorporateOfficer"/>
      <rdfs:range rdf:resource="http://www.omg.org/spec/EDMC-SR/BE/LegalEntities/LegalPersons/NaturalPerson"/>
   </owl:ObjectProperty>

   <owl:ObjectProperty rdf:about="http://www.omg.org/spec/EDMC-SR/BE/OwnershipAndControl/Executives/corporateOfficerHasResponsibility">
      <skos:definition>The Company Public Officer is party to some statutory obligations as mandated by the applicable body of Company Law.</skos:definition>
      <rdfs:subPropertyOf rdf:resource="http://www.omg.org/spec/EDMC-SR/BE/OwnershipAndControl/Executives/responsiblePartyHasResponsibility"/>
      <rdfs:domain rdf:resource="http://www.omg.org/spec/EDMC-SR/BE/OwnershipAndControl/Executives/CorporateOfficer"/>
      <rdfs:range rdf:resource="http://www.omg.org/spec/EDMC-SR/BE/OwnershipAndControl/Executives/CompanyStatutoryObligation"/>
   </owl:ObjectProperty>

   <owl:ObjectProperty rdf:about="http://www.omg.org/spec/EDMC-SR/BE/OwnershipAndControl/Executives/corporateOfficerHasResponsibilityDuty">
      <skos:definition>The Company Public Officer is party to some formally defined Public Officer Duty as set out on the relevant piece of Company Law.</skos:definition>
      <rdfs:subPropertyOf rdf:resource="http://www.omg.org/spec/EDMC-SR/BE/OwnershipAndControl/Executives/responsiblePartyHasResponsibility"/>
      <rdfs:domain rdf:resource="http://www.omg.org/spec/EDMC-SR/BE/OwnershipAndControl/Executives/CorporateOfficer"/>
      <rdfs:range rdf:resource="http://www.omg.org/spec/EDMC-SR/BE/OwnershipAndControl/Executives/CorporateOfficerDuty"/>
   </owl:ObjectProperty>

   <owl:ObjectProperty rdf:about="http://www.omg.org/spec/EDMC-SR/BE/OwnershipAndControl/Executives/deFactoControllingInterestPartyAppoints">
      <skos:definition>The Control Owner has some mechanism whereby they are able to vote and approve the board, other than through the mechanisms defined elsewhere.</skos:definition>
      <skos:editorialNote>The Board Members appoint Public Officers. The Public Officers are not necessarily exclusively responsible to the Board. All management control is delegated from the Board on behalf of the Shareholders.</skos:editorialNote>
      <rdfs:subPropertyOf rdf:resource="http://www.omg.org/spec/EDMC-SR/FND/Relations/Relations/appoints"/>
      <rdfs:domain rdf:resource="http://www.omg.org/spec/EDMC-SR/BE/OwnershipAndControl/ControlParties/DeFactoControllingInterestParty"/>
      <rdfs:range rdf:resource="http://www.omg.org/spec/EDMC-SR/BE/OwnershipAndControl/Executives/BoardMember"/>
   </owl:ObjectProperty>

   <owl:ObjectProperty rdf:about="http://www.omg.org/spec/EDMC-SR/BE/OwnershipAndControl/Executives/directorHasIdentity">
      <skos:definition>A board member (director) is typically a Natural Person, but may be any Legal Person.</skos:definition>
      <skos:editorialNote>Board Member is synonymous with Director. In most jurisdictions e.g. those in the US, a director has to be a natural person. in the UK only an Incorporated Company or a natural person can be a board member. That is, if you are NOT a Natural Person, you have to be one of a very small sub-set of types of legal person namely anything which is legally Incorporated (any Body Corporate in this model).</skos:editorialNote>
      <rdfs:subPropertyOf rdf:resource="http://www.omg.org/spec/EDMC-SR/FND/Parties/Parties/partyInRoleHasIdentity"/>
      <rdfs:subPropertyOf rdf:resource="http://www.omg.org/spec/EDMC-SR/BE/OwnershipAndControl/Executives/legallyDelegatedAuthorityHasIdentity"/>
      <rdfs:domain rdf:resource="http://www.omg.org/spec/EDMC-SR/BE/OwnershipAndControl/Executives/BoardMember"/>
      <rdfs:range rdf:resource="http://www.omg.org/spec/EDMC-SR/BE/LegalEntities/LegalPersons/LegalPerson"/>
   </owl:ObjectProperty>

   <owl:ObjectProperty rdf:about="http://www.omg.org/spec/EDMC-SR/BE/OwnershipAndControl/Executives/executiveIdentity">
      <skos:definition>The Executive is some adult human being.</skos:definition>
      <rdfs:subPropertyOf rdf:resource="http://www.omg.org/spec/EDMC-SR/BE/OwnershipAndControl/Executives/legallyDelegatedAuthorityHasIdentity"/>
      <rdfs:domain rdf:resource="http://www.omg.org/spec/EDMC-SR/BE/OwnershipAndControl/Executives/Executive"/>
      <rdfs:range rdf:resource="http://www.omg.org/spec/EDMC-SR/BE/LegalEntities/LegalPersons/NaturalPerson"/>
   </owl:ObjectProperty>

   <owl:ObjectProperty rdf:about="http://www.omg.org/spec/EDMC-SR/BE/OwnershipAndControl/Executives/legallyDelegatedAuthorityHasIdentity">
      <skos:definition>That which is in the role of Legally Controlling Party. This must be a Legal Person.</skos:definition>
      <rdfs:subPropertyOf rdf:resource="http://www.omg.org/spec/EDMC-SR/FND/Parties/Parties/partyInRoleHasIdentity"/>
      <rdfs:domain rdf:resource="http://www.omg.org/spec/EDMC-SR/BE/OwnershipAndControl/Executives/LegallyDelegatedAuthority"/>
      <rdfs:range rdf:resource="http://www.omg.org/spec/EDMC-SR/BE/LegalEntities/LegalPersons/LegalPerson"/>
   </owl:ObjectProperty>

   <owl:ObjectProperty rdf:about="http://www.omg.org/spec/EDMC-SR/BE/OwnershipAndControl/Executives/responsiblePartyIdentity">
      <skos:definition>The Responsible Party must be some Natural Person.</skos:definition>
      <skos:editorialNote>This is the kind of party for whom specific responsibilities are set out in law, and which must be natural persons charged with those responsibilities on behalf of some entity.</skos:editorialNote>
      <rdfs:subPropertyOf rdf:resource="http://www.omg.org/spec/EDMC-SR/FND/Parties/Parties/partyInRoleHasIdentity"/>
      <rdfs:domain rdf:resource="http://www.omg.org/spec/EDMC-SR/BE/OwnershipAndControl/Executives/ResponsibleParty"/>
      <rdfs:range rdf:resource="http://www.omg.org/spec/EDMC-SR/BE/LegalEntities/LegalPersons/NaturalPerson"/>
   </owl:ObjectProperty>

   <owl:ObjectProperty rdf:about="http://www.omg.org/spec/EDMC-SR/BE/OwnershipAndControl/Executives/responsiblePartyHasResponsibility">
      <skos:definition>The Responsible Party is deemed to be such because it is party to some formally defined Duty.</skos:definition>
      <rdfs:subPropertyOf rdf:resource="http://www.omg.org/spec/EDMC-SR/BE/OwnershipAndControl/Executives/hasReponsibility"/>
      <rdfs:domain rdf:resource="http://www.omg.org/spec/EDMC-SR/BE/OwnershipAndControl/Executives/ResponsibleParty"/>
      <rdfs:range rdf:resource="http://www.omg.org/spec/EDMC-SR/FND/Law/LegalCapacities/Duty"/>
   </owl:ObjectProperty>

   <owl:ObjectProperty rdf:about="http://www.omg.org/spec/EDMC-SR/BE/OwnershipAndControl/Executives/votingShareholderElects">
      <skos:definition>The shareholders approve and vote for the members of the Board.</skos:definition>
      <skos:editorialNote>The bylaws give the manner in which that process is effected. The candidate members may be suggested by the Board and are then voted for by the Shareholder. There is typically a committee for trustees or something, to do that.</skos:editorialNote>
      <rdfs:subPropertyOf rdf:resource="http://www.omg.org/spec/EDMC-SR/BE/OwnershipAndControl/Executives/elects"/>
      <rdfs:domain rdf:resource="http://www.omg.org/spec/EDMC-SR/BE/OwnershipAndControl/CorporateControl/VotingShareholder"/>
      <rdfs:range rdf:resource="http://www.omg.org/spec/EDMC-SR/BE/OwnershipAndControl/Executives/BoardMember"/>
   </owl:ObjectProperty>

   <owl:ObjectProperty rdf:about="http://www.omg.org/spec/EDMC-SR/BE/OwnershipAndControl/Executives/delegatesControlTo">
      <skos:definition>The Organization which has management control of this Organization.</skos:definition>
      <rdfs:subPropertyOf rdf:resource="http://www.omg.org/spec/EDMC-SR/FND/Relations/Relations/designates"/>
      <rdfs:domain rdf:resource="http://www.omg.org/spec/EDMC-SR/BE/LegalEntities/LegalPersons/LegalPerson"/>
      <rdfs:range rdf:resource="http://www.omg.org/spec/EDMC-SR/BE/OwnershipAndControl/Executives/LegallyDelegatedAuthority"/>
   </owl:ObjectProperty>

   <owl:ObjectProperty rdf:about="http://www.omg.org/spec/EDMC-SR/BE/OwnershipAndControl/Executives/elects">
      <rdfs:subPropertyOf rdf:resource="http://www.omg.org/spec/EDMC-SR/FND/Relations/Relations/designates"/>
      <rdfs:domain rdf:resource="http://www.omg.org/spec/EDMC-SR/BE/LegalEntities/LegalPersons/LegalPerson"/>
      <rdfs:range rdf:resource="http://www.omg.org/spec/EDMC-SR/BE/LegalEntities/LegalPersons/LegalPerson"/>
   </owl:ObjectProperty>

   <owl:ObjectProperty rdf:about="http://www.omg.org/spec/EDMC-SR/BE/OwnershipAndControl/Executives/hasCapacityCorporateOfficerCapacity">
      <skos:definition>The public officer of a company has some formal capacity vested in them.</skos:definition>
      <rdfs:subPropertyOf rdf:resource="http://www.omg.org/spec/EDMC-SR/FND/Law/LegalCapacities/hasCapacity"/>
      <rdfs:domain rdf:resource="http://www.omg.org/spec/EDMC-SR/BE/OwnershipAndControl/Executives/CorporateOfficer"/>
      <rdfs:range rdf:resource="http://www.omg.org/spec/EDMC-SR/BE/OwnershipAndControl/Executives/CorporateOfficerCapacity"/>
   </owl:ObjectProperty>

   <owl:ObjectProperty rdf:about="http://www.omg.org/spec/EDMC-SR/BE/OwnershipAndControl/Executives/hasCapacitySignatoryCapacity">
      <skos:definition>The party which is a Company Public Officer is also defined as being a signatory in respect of the entity, that is the officer is able to sign agreements on the part of that entity.</skos:definition>
      <rdfs:subPropertyOf rdf:resource="http://www.omg.org/spec/EDMC-SR/FND/Law/LegalCapacities/hasCapacity"/>
      <rdfs:domain rdf:resource="http://www.omg.org/spec/EDMC-SR/BE/OwnershipAndControl/Executives/CorporateOfficer"/>
      <rdfs:range rdf:resource="http://www.omg.org/spec/EDMC-SR/FND/Law/LegalCapacities/SignatoryCapacity"/>
   </owl:ObjectProperty>

   <owl:ObjectProperty rdf:about="http://www.omg.org/spec/EDMC-SR/BE/OwnershipAndControl/Executives/hasDelegatedControlOf">
      <skos:definition>An organization of which this organization has control via some management structure.</skos:definition>
      <skos:editorialNote>Any distinction between board level voting rights control versus managerial control is not part of this definition.</skos:editorialNote>
      <rdfs:domain rdf:resource="http://www.omg.org/spec/EDMC-SR/BE/OwnershipAndControl/Executives/LegallyDelegatedAuthority"/>
      <rdfs:range rdf:resource="http://www.omg.org/spec/EDMC-SR/BE/LegalEntities/LegalPersons/LegalPerson"/>
   </owl:ObjectProperty>

   <owl:ObjectProperty rdf:about="http://www.omg.org/spec/EDMC-SR/BE/OwnershipAndControl/Executives/hasDelegatedControlOfItself">
      <rdfs:domain rdf:resource="http://www.omg.org/spec/EDMC-SR/BE/OwnershipAndControl/Executives/LegallyDelegatedAuthority"/>
      <rdfs:range rdf:resource="http://www.omg.org/spec/EDMC-SR/BE/LegalEntities/LegalPersons/LegalPerson"/>
      <owl:inverseOf rdf:resource="http://www.omg.org/spec/EDMC-SR/BE/OwnershipAndControl/Executives/delegatesControlTo"/>
   </owl:ObjectProperty>

   <owl:ObjectProperty rdf:about="http://www.omg.org/spec/EDMC-SR/BE/OwnershipAndControl/Executives/hasReponsibility">
      <rdfs:domain rdf:resource="http://www.omg.org/spec/EDMC-SR/FND/Relations/Relations/Thing"/>
      <rdfs:range rdf:resource="http://www.omg.org/spec/EDMC-SR/FND/Law/LegalCapacities/Duty"/>
   </owl:ObjectProperty>

   <owl:ObjectProperty rdf:about="http://www.omg.org/spec/EDMC-SR/BE/OwnershipAndControl/Executives/hasResponsibleParty">
      <skos:definition>Some party having some defined responsibility in respect of the Formal Organization</skos:definition>
      <rdfs:subPropertyOf rdf:resource="http://www.omg.org/spec/EDMC-SR/FND/Parties/Parties/hasPartyInRole"/>
      <rdfs:domain rdf:resource="http://www.omg.org/spec/EDMC-SR/FND/Organizations/FormalOrganizations/FormalOrganization"/>
      <rdfs:range rdf:resource="http://www.omg.org/spec/EDMC-SR/BE/OwnershipAndControl/Executives/ResponsibleParty"/>
   </owl:ObjectProperty>

   <owl:ObjectProperty rdf:about="http://www.omg.org/spec/EDMC-SR/BE/OwnershipAndControl/Executives/hasVestedInIt">
      <skos:definition>A Delegated Legal Authority is one which has the legal capacity of Delegated Legal Authority vested in it.</skos:definition>
      <rdfs:subPropertyOf rdf:resource="http://www.omg.org/spec/EDMC-SR/FND/Law/LegalCapacities/hasCapacity"/>
      <rdfs:domain rdf:resource="http://www.omg.org/spec/EDMC-SR/BE/OwnershipAndControl/Executives/LegallyDelegatedAuthority"/>
      <rdfs:range rdf:resource="http://www.omg.org/spec/EDMC-SR/FND/Law/LegalCapacities/DelegatedLegalAuthority"/>
   </owl:ObjectProperty>

   <owl:ObjectProperty rdf:about="http://www.omg.org/spec/EDMC-SR/BE/OwnershipAndControl/Executives/mandatedByCompanyLaw">
      <skos:definition>The duties of a Company Public Officer are mandated by some applicable piece of Company Law.</skos:definition>
      <rdfs:subPropertyOf rdf:resource="http://www.omg.org/spec/EDMC-SR/BE/OwnershipAndControl/Executives/mandatedBy"/>
      <rdfs:domain rdf:resource="http://www.omg.org/spec/EDMC-SR/BE/OwnershipAndControl/Executives/CorporateOfficerDuty"/>
      <rdfs:range rdf:resource="http://www.omg.org/spec/EDMC-SR/BE/OwnershipAndControl/Executives/CompanyLaw"/>
   </owl:ObjectProperty>

   <!--Data Properties-->

<!--Annotation Properties-->

<!--Classes-->

<owl:Class rdf:about="http://www.omg.org/spec/EDMC-SR/BE/OwnershipAndControl/Executives/Anon-19003">
      <skos:definition>The logical union of company legal form documents (Instrument of Incorporation, Memorandum and Articles or equivalent) and company by-laws.</skos:definition>
      <owl:equivalentClass>
         <owl:Class>
            <owl:unionOf rdf:parseType="Collection">
               <owl:Class rdf:about="http://www.omg.org/spec/EDMC-SR/BE/LegalEntities/CorporateBodies/InstrumentOfIncorporation"/>
               <owl:Class rdf:about="http://www.omg.org/spec/EDMC-SR/BE/Corporations/Corporations/BoardAgreement"/>
               <owl:Class rdf:about="http://www.omg.org/spec/EDMC-SR/BE/OwnershipAndControl/Executives/CompanyBylaw"/>
            </owl:unionOf>
         </owl:Class>
      </owl:equivalentClass>
   </owl:Class>

   <owl:Class rdf:about="http://www.omg.org/spec/EDMC-SR/BE/OwnershipAndControl/Executives/ArticlesOfIncorporation">
      <rdfs:label>Articles Of Incorporation</rdfs:label>
      <skos:definition>The Articles of Association are a contract between the members and the organization, and among the members themselves, setting out the rights and duties of directors and stockholders individually and in meetings. Editorial Note: New definition and term (added in Executives) arrived at during OMG OWL migration process. Known then as "Incorporated Company Legal form Documentation" (seeking a jurisdiction neutral label). Original working definition: "The articles of association which are defined when a registered company (specifically a company limited by the issue of shares) is set up. " Explanatory Note: In some (or all?) Jurisdictions the articles in the company constitution become terms of the contract which is a share in that company. Example: In the UK: Memorandum and Articles of Association make up the Constitution. Bits of that are defined by law. In Delaware you have to have 3 officers which may be the same individual. Other states they must be separate individuals. Also in Delaware they need not be American citizens, in other states they must. Minimum requirements to be met. Also this may change as law changes. See also Anti ML and KYC stuff. Schools - governing bodies, their constitutions. Trusts.</skos:definition>
      <rdfs:subClassOf rdf:resource="http://www.omg.org/spec/EDMC-SR/BE/LegalEntities/CorporateBodies/InstrumentOfIncorporation"/>
   </owl:Class>

   <owl:Class rdf:about="http://www.omg.org/spec/EDMC-SR/BE/OwnershipAndControl/Executives/Auditor">
      <rdfs:label>Auditor</rdfs:label>
      <skos:definition>The auditor of the company is a public officer which is responsible for reporting on the financial situation of the company.</skos:definition>
      <skos:editorialNote>They have power independently of the board. Power to assess the quality of the financial reports. Also has obligations to the statutory authorities in that regard. The auditor has obligations to the shareholders which are not directly to the Board. Their specific role is to supervise the board to ensure they are acting on behalf of the shareholders. To report to the shareholders on the activities of the Board. Therefore, Auditor's report is a required part of the financial reports. They are responsible for providing a "true and fair view" of the financial positions of the company. Election: Put up by the board. Appointed by the Board on behalf of the shareholders. Can be voted out by the shareholders at an AGM or EGM but the board can also put up a competitive process. Normally board elects them but the shareholders can override that selection. HistoryNote: This last note below is from when this was still defined as a kind of Company Public Officer before we renamed that to Corporate Officer and made it an internal oofficer only: In general, Public Officers are appointed by the Board but can ultimately be overridden by the shareholders acting as a group. the board is their representatives.</skos:editorialNote>
      <rdfs:subClassOf rdf:resource="http://www.omg.org/spec/EDMC-SR/BE/OwnershipAndControl/Executives/ResponsibleParty"/>
   </owl:Class>

   <owl:Class rdf:about="http://www.omg.org/spec/EDMC-SR/BE/OwnershipAndControl/Executives/BoardCapacity">
      <rdfs:label>Board Capacity</rdfs:label>
      <skos:definition>The capacity which resides in the Board of Directors of a company.</skos:definition>
      <rdfs:subClassOf rdf:resource="http://www.omg.org/spec/EDMC-SR/FND/Law/LegalCapacities/DelegatedLegalAuthority"/>
   </owl:Class>

   <owl:Class rdf:about="http://www.omg.org/spec/EDMC-SR/BE/OwnershipAndControl/Executives/BoardMember">
      <rdfs:label>Board Member</rdfs:label>
      <skos:definition>A person who is a member of the Board of Directors of some Incorporated company.</skos:definition>
      <skos:editorialNote>Define sub-types e.g. executive and non executive board member May include independents who come in from other companies. Legal responsibilities of Board Member. Example: allegation that corp has misappropriated funds. Then company officers are sued not just any board member. However, if corporation is sued they are liable. Would be going after officers specifically because of their responsibilities, but can also go after the corporation whereof the board members are responsible. See "Piercing the corporate veil".SarbOx etc.</skos:editorialNote>
      <rdfs:subClassOf rdf:resource="http://www.omg.org/spec/EDMC-SR/BE/OwnershipAndControl/Executives/LegallyDelegatedAuthority"/>
      <rdfs:subClassOf rdf:resource="http://www.omg.org/spec/EDMC-SR/FND/Parties/Parties/OrganizationMember"/>
   </owl:Class>

   <owl:Class rdf:about="http://www.omg.org/spec/EDMC-SR/BE/OwnershipAndControl/Executives/BoardOfDirectors">
      <rdfs:label>Board Of Directors</rdfs:label>
      <skos:definition>The group of entities defined as being the Board of Directors of the company.</skos:definition>
      <rdfs:subClassOf rdf:resource="http://www.omg.org/spec/EDMC-SR/BE/OwnershipAndControl/ControlParties/EntityControllingParty"/>
   </owl:Class>

   <owl:Class rdf:about="http://www.omg.org/spec/EDMC-SR/BE/OwnershipAndControl/Executives/Bylaw">
      <rdfs:label>Bylaw</rdfs:label>
      <skos:definition>The bylaws of some commercial or other registered enterprise.</skos:definition>
      <rdfs:subClassOf rdf:resource="http://www.omg.org/spec/EDMC-SR/FND/Law/LegalCore/Law"/>
   </owl:Class>

   <owl:Class rdf:about="http://www.omg.org/spec/EDMC-SR/BE/OwnershipAndControl/Executives/ChiefExecutiveOfficer">
      <rdfs:label>Chief Executive Officer</rdfs:label>
      <skos:definition>Some person performing the role of Chief Executive Officer of a company, with the responsibilities and rights defined for that party in the relevant statutes.</skos:definition>
      <rdfs:subClassOf rdf:resource="http://www.omg.org/spec/EDMC-SR/BE/OwnershipAndControl/Executives/CorporateOfficer"/>
      <rdfs:subClassOf rdf:resource="http://www.omg.org/spec/EDMC-SR/BE/OwnershipAndControl/Executives/ExecutiveBoardMember"/>
   </owl:Class>

   <owl:Class rdf:about="http://www.omg.org/spec/EDMC-SR/BE/OwnershipAndControl/Executives/ChiefFinancialOfficer">
      <rdfs:label>Chief Financial Officer</rdfs:label>
      <skos:definition>Some person performing the role of Chief Financial Officer of a company, with the responsibilities and rights defined for that party in the relevant statutes.</skos:definition>
      <rdfs:subClassOf rdf:resource="http://www.omg.org/spec/EDMC-SR/BE/OwnershipAndControl/Executives/Executive"/>
   </owl:Class>

   <owl:Class rdf:about="http://www.omg.org/spec/EDMC-SR/BE/OwnershipAndControl/Executives/CompanyBylaw">
      <rdfs:label>Company Bylaw</rdfs:label>
      <skos:definition>A by-law of a company.</skos:definition>
      <rdfs:subClassOf rdf:resource="http://www.omg.org/spec/EDMC-SR/BE/OwnershipAndControl/Executives/Bylaw"/>
   </owl:Class>

   <owl:Class rdf:about="http://www.omg.org/spec/EDMC-SR/BE/OwnershipAndControl/Executives/CompanyLaw">
      <rdfs:label>Company Law</rdfs:label>
      <skos:definition>The law dealing with companies in a given jurisdiction.</skos:definition>
      <rdfs:subClassOf rdf:resource="http://www.omg.org/spec/EDMC-SR/FND/Law/Jurisdictions/StatuteLaw"/>
   </owl:Class>

   <owl:Class rdf:about="http://www.omg.org/spec/EDMC-SR/BE/OwnershipAndControl/Executives/CompanySecretary">
      <rdfs:label>Company Secretary</rdfs:label>
      <skos:definition>Formal definition required</skos:definition>
      <skos:editorialNote>Functionary but also a signer of documentation in the company. Does not have powers to do anything without instruction from the board. THe rol arsies from legal obligations iposed by the company. responsible to legislative authorities fo rthe company meeting those legal obligations. Role is that they gain a degree of control but only in the fact that they must report according to rules established by theirlegislative jurisdiction. Example: Delaware: you need a designated corporate secretary who is responsible for submitting certain documents etc.</skos:editorialNote>
   </owl:Class>

   <owl:Class rdf:about="http://www.omg.org/spec/EDMC-SR/BE/OwnershipAndControl/Executives/CompanyStatutoryObligation">
      <rdfs:label>Company Statutory Obligation</rdfs:label>
      <skos:definition>An obligation defined in company law (statute).</skos:definition>
      <skos:editorialNote>This is the set of laws that define the statutory obligations on public officers for the jurisdiction in which the company operates.</skos:editorialNote>
      <rdfs:subClassOf rdf:resource="http://www.omg.org/spec/EDMC-SR/FND/Law/LegalCapacities/StatutoryResponsibility"/>
   </owl:Class>

   <owl:Class rdf:about="http://www.omg.org/spec/EDMC-SR/BE/OwnershipAndControl/Executives/CorporateOfficer">
      <rdfs:label>Corporate Officer</rdfs:label>
      <skos:definition>Some party which is recognized by law as having the role and responsibilities defined for a Public Officer as described in that law.</skos:definition>
   </owl:Class>

   <owl:Class rdf:about="http://www.omg.org/spec/EDMC-SR/BE/OwnershipAndControl/Executives/CorporateOfficerCapacity">
      <rdfs:label>Corporate Officer Capacity</rdfs:label>
      <skos:definition>The capacity vested in a public officer of a company. Further notes: This is framed as a capacity: Individual acts in their capacity of the role as CFO, CEO etc. but their legal liability rests in their relationship with the board itself i.e. comes from their membership on the board from a corporate standpoint. Scope Note: Originally framed with reference to Incorporated company, this term and its related terms have been re-framed as applying to any Body Corporate. May be specialized for Incorporated Companies and other Bodies Corporate at some future point.</skos:definition>
   </owl:Class>

   <owl:Class rdf:about="http://www.omg.org/spec/EDMC-SR/BE/OwnershipAndControl/Executives/CorporateOfficerDuty">
      <rdfs:label>Corporate Officer Duty</rdfs:label>
      <skos:definition>Some duty incumbent upon some public officer of a company.</skos:definition>
      <rdfs:subClassOf rdf:resource="http://www.omg.org/spec/EDMC-SR/BE/OwnershipAndControl/Executives/CompanyStatutoryObligation"/>
   </owl:Class>

   <owl:Class rdf:about="http://www.omg.org/spec/EDMC-SR/BE/OwnershipAndControl/Executives/Executive">
      <rdfs:label>Executive</rdfs:label>
      <skos:definition>Some person in whom some level of management control of some organization has been conferred. Further Notes The owners of a business delegate their controlling parties ot controlling parties which gives them the right to control. These rights are reassigned by the creditors in the event of a business being under receivership.</skos:definition>
   </owl:Class>

   <owl:Class rdf:about="http://www.omg.org/spec/EDMC-SR/BE/OwnershipAndControl/Executives/ExecutiveBoardMember">
      <rdfs:label>Executive Board Member</rdfs:label>
      <skos:definition>Some person performing the role of a Board Member of a company, and being one with some executive responsibilities within that company.</skos:definition>
      <rdfs:subClassOf rdf:resource="http://www.omg.org/spec/EDMC-SR/BE/OwnershipAndControl/Executives/BoardMember"/>
   </owl:Class>

   <owl:Class rdf:about="http://www.omg.org/spec/EDMC-SR/BE/OwnershipAndControl/Executives/LegallyDelegatedAuthority">
      <rdfs:label>Legally Delegated Authority</rdfs:label>
      <skos:definition>A party having some legal control of some entity.</skos:definition>
      <rdfs:subClassOf rdf:resource="http://www.omg.org/spec/EDMC-SR/FND/OwnershipAndControl/Control/ControllingParty"/>
   </owl:Class>

   <owl:Class rdf:about="http://www.omg.org/spec/EDMC-SR/BE/OwnershipAndControl/Executives/NonExecutiveBoardMember">
      <rdfs:label>Non Executive Board Member</rdfs:label>
      <skos:definition>Some person performing the role of a Board Member of a company, and having no executive responsibilities towards the running of the company.</skos:definition>
   </owl:Class>

   <owl:Class rdf:about="http://www.omg.org/spec/EDMC-SR/BE/OwnershipAndControl/Executives/ResponsibleParty">
      <rdfs:label>Responsible Party</rdfs:label>
      <skos:definition>A Party to which some responsibility has been given.</skos:definition>
      <skos:editorialNote>The responsibility may be defined in terms of specific instruments such as laws, by-laws or contracts, or by some other means. These instruments would mandate certain obligations on the part of the party, for example statutory obligations. REVIEW QUESTIONS: - Should we distinguish "Statutory" obligations from others (these being obligations defined by statute)? - Is there a range of kinds of responsible party, or only those with statury obligations? How best to taxonomize these .</skos:editorialNote>
      <rdfs:subClassOf rdf:resource="http://www.omg.org/spec/EDMC-SR/FND/Parties/Parties/PartyInRole"/>
   </owl:Class>

   <!--Individuals-->

</rdf:RDF>