<?xml version="1.0" encoding="UTF-8"?>
  
<!DOCTYPE rdf:RDF [
    <!ENTITY fibo-fnd-bus-bg "http://spec.edmcouncil.org/fibo/red/fnd/business/business-goals/">
    <!ENTITY fibo-fnd-gao-gl "http://spec.edmcouncil.org/fibo/red/fnd/goals-and-objectives/goals/">
]>

<rdf:RDF xmlns:xsd="http://www.w3.org/2001/XMLSchema#"
         xmlns:sm="http://www.omg.org/techprocess/ab/SpecificationMetadata/"
         xmlns:xs="http://www.w3.org/2001/XMLSchema"
         xmlns:fibo-fnd-utl-av="http://www.omg.org/spec/EDMC-FIBO/FND/Utilities/AnnotationVocabulary/"
         xmlns:rdf="http://www.w3.org/1999/02/22-rdf-syntax-ns#"
         xmlns:rdfs="http://www.w3.org/2000/01/rdf-schema#"
         xmlns:owl="http://www.w3.org/2002/07/owl#"
         xmlns:skos="http://www.w3.org/2004/02/skos/core#"
         xmlns:dc="http://purl.org/dc/terms/"
         xml:base="http://spec.edmcouncil.org/fibo/red/fnd/business/business-goals/">

   <owl:Ontology rdf:about="http://spec.edmcouncil.org/fibo/red/fnd/business/business-goals/">
      <owl:imports rdf:resource="http://spec.edmcouncil.org/fibo/red/fnd/goals-and-objectives/goals/"/>
   </owl:Ontology>


  <!--
    ///////////////////////////////////////////////////////////////////////////////////////
    //
    // Datatypes
    //
    ///////////////////////////////////////////////////////////////////////////////////////
    -->



  <!--
    ///////////////////////////////////////////////////////////////////////////////////////
    //
    // Object Properties
    //
    ///////////////////////////////////////////////////////////////////////////////////////
    -->



  <!--
    ///////////////////////////////////////////////////////////////////////////////////////
    //
    // Data Properties
    //
    ///////////////////////////////////////////////////////////////////////////////////////
    -->



  <!--
    ///////////////////////////////////////////////////////////////////////////////////////
    //
    // Annotation Properties
    //
    ///////////////////////////////////////////////////////////////////////////////////////
    -->



  <!--
    ///////////////////////////////////////////////////////////////////////////////////////
    //
    // Classes
    //
    ///////////////////////////////////////////////////////////////////////////////////////
    -->


<owl:Class rdf:about="&fibo-fnd-bus-bg;BusinessGoal">
      <rdfs:label>business goal</rdfs:label>
      <skos:definition>A Goal is a state or condition of the enterprise to be brought about or sustained through appropriate Means.</skos:definition>
      <rdfs:subClassOf rdf:resource="&fibo-fnd-gao-gl;Goal"/>
   </owl:Class>

   <owl:Class rdf:about="&fibo-fnd-bus-bg;CorporateGoal">
      <rdfs:label>corporate goal</rdfs:label>
      <skos:definition>A business goal in the furtherance of the aims and profitability of a corporation.</skos:definition>
      <rdfs:subClassOf rdf:resource="&fibo-fnd-bus-bg;BusinessGoal"/>
   </owl:Class>

   <owl:Class rdf:about="&fibo-fnd-bus-bg;FinancialWellbeing">
      <rdfs:label>financial wellbeing</rdfs:label>
      <skos:definition>The overall balance sheet and well being of the organisation.</skos:definition>
      <rdfs:subClassOf rdf:resource="&fibo-fnd-bus-bg;InvestmentGoal"/>
   </owl:Class>

   <owl:Class rdf:about="&fibo-fnd-bus-bg;InvestmentGoal">
      <rdfs:label>investment goal</rdfs:label>
      <skos:definition>A goal for which is to be achieved by investments within an investment institution.</skos:definition>
   </owl:Class>

   <owl:Class rdf:about="&fibo-fnd-bus-bg;LendingGoal">
      <rdfs:label>lending goal</rdfs:label>
      <skos:definition>Reasons for extending loans and credit, i.e. the organisation has a goal to create capital growth by extending credit or making loans.</skos:definition>
   </owl:Class>

   <owl:Class rdf:about="&fibo-fnd-bus-bg;MarketInvestmentGoal">
      <rdfs:label>market investment goal</rdfs:label>
      <skos:definition>A business goal driving investment activities as distinct from day to day commercial trading activities.</skos:definition>
   </owl:Class>

   <owl:Class rdf:about="&fibo-fnd-bus-bg;ProjectGoal">
      <rdfs:label>project goal</rdfs:label>
      <skos:definition>Some stated goal of a project as set out in the project planning documentation.</skos:definition>
   </owl:Class>

   <owl:Class rdf:about="&fibo-fnd-bus-bg;Reputation">
      <rdfs:label>reputation</rdfs:label>
      <skos:definition>The goal of a business to maintain or enhance its reputation.</skos:definition>
   </owl:Class>

   <owl:Class rdf:about="&fibo-fnd-bus-bg;TransactionProcessingGoal">
      <rdfs:label>transaction processing goal</rdfs:label>
      <skos:definition>The goal of processing transactions in which the organization is engaged, without error and within the stated time constraints.</skos:definition>
   </owl:Class>


  <!--
    ///////////////////////////////////////////////////////////////////////////////////////
    //
    // Individuals
    //
    ///////////////////////////////////////////////////////////////////////////////////////
    -->


</rdf:RDF>