<?xml version="1.0" encoding="UTF-8"?>
<!DOCTYPE rdf:RDF [
	<!ENTITY dct "http://purl.org/dc/terms/">
	<!ENTITY fibo-der-ass-ass "https://spec.edmcouncil.org/fibo/ontology/DER/AssetDerivatives/AssetDerivatives/">
	<!ENTITY fibo-der-ass-eqf "https://spec.edmcouncil.org/fibo/ontology/DER/AssetDerivatives/EquityForwards/">
	<!ENTITY fibo-der-ass-eqs "https://spec.edmcouncil.org/fibo/ontology/DER/AssetDerivatives/EquitySwaps/">
	<!ENTITY fibo-der-der-fwd "https://spec.edmcouncil.org/fibo/ontology/DER/DerivativesContracts/Forwards/">
	<!ENTITY fibo-fnd-acc-cur "https://spec.edmcouncil.org/fibo/ontology/FND/Accounting/CurrencyAmount/">
	<!ENTITY fibo-fnd-dt-fd "https://spec.edmcouncil.org/fibo/ontology/FND/DatesAndTimes/FinancialDates/" >
	<!ENTITY fibo-fnd-arrxx-meth "https://spec.edmcouncil.org/fibo/ontology/FND/ArrangementsExt/MethodsAndRules/">
	<!ENTITY fibo-fnd-utl-av "https://spec.edmcouncil.org/fibo/ontology/FND/Utilities/AnnotationVocabulary/">
	<!ENTITY owl "http://www.w3.org/2002/07/owl#">
	<!ENTITY rdf "http://www.w3.org/1999/02/22-rdf-syntax-ns#">
	<!ENTITY rdfs "http://www.w3.org/2000/01/rdf-schema#">
	<!ENTITY skos "http://www.w3.org/2004/02/skos/core#">
	<!ENTITY xsd "http://www.w3.org/2001/XMLSchema#">
]>
<rdf:RDF xml:base="https://spec.edmcouncil.org/fibo/ontology/DER/AssetDerivatives/EquityForwards/"
	xmlns:dct="http://purl.org/dc/terms/"
	xmlns:fibo-der-ass-ass="https://spec.edmcouncil.org/fibo/ontology/DER/AssetDerivatives/AssetDerivatives/"
	xmlns:fibo-der-ass-eqf="https://spec.edmcouncil.org/fibo/ontology/DER/AssetDerivatives/EquityForwards/"
	xmlns:fibo-der-ass-eqs="https://spec.edmcouncil.org/fibo/ontology/DER/AssetDerivatives/EquitySwaps/"
	xmlns:fibo-der-der-fwd="https://spec.edmcouncil.org/fibo/ontology/DER/DerivativesContracts/Forwards/"
	xmlns:fibo-fnd-acc-cur="https://spec.edmcouncil.org/fibo/ontology/FND/Accounting/CurrencyAmount/"
	xmlns:fibo-fnd-dt-fd="https://spec.edmcouncil.org/fibo/ontology/FND/DatesAndTimes/FinancialDates/"
	xmlns:fibo-fnd-arrxx-meth="https://spec.edmcouncil.org/fibo/ontology/FND/ArrangementsExt/MethodsAndRules/"
	xmlns:fibo-fnd-utl-av="https://spec.edmcouncil.org/fibo/ontology/FND/Utilities/AnnotationVocabulary/"
	xmlns:owl="http://www.w3.org/2002/07/owl#"
	xmlns:rdf="http://www.w3.org/1999/02/22-rdf-syntax-ns#"
	xmlns:rdfs="http://www.w3.org/2000/01/rdf-schema#"
	xmlns:skos="http://www.w3.org/2004/02/skos/core#"
	xmlns:xsd="http://www.w3.org/2001/XMLSchema#">
	
	<owl:Ontology rdf:about="https://spec.edmcouncil.org/fibo/ontology/DER/AssetDerivatives/EquityForwards/">
		<rdfs:label xml:lang="en">EquityForwards</rdfs:label>
		<dct:abstract>Forward contracts based on an underlying equity instrument.</dct:abstract>
		<owl:imports rdf:resource="https://spec.edmcouncil.org/fibo/ontology/DER/AssetDerivatives/AssetDerivatives/"/>
		<owl:imports rdf:resource="https://spec.edmcouncil.org/fibo/ontology/DER/AssetDerivatives/EquitySwaps/"/>
		<owl:imports rdf:resource="https://spec.edmcouncil.org/fibo/ontology/DER/DerivativesContracts/DerivativesBasics/"/>
		<owl:imports rdf:resource="https://spec.edmcouncil.org/fibo/ontology/DER/DerivativesContracts/Forwards/"/>
		<owl:imports rdf:resource="https://spec.edmcouncil.org/fibo/ontology/FBC/FinancialInstruments/FinancialInstruments/"/>
		<owl:imports rdf:resource="https://spec.edmcouncil.org/fibo/ontology/FND/Accounting/CurrencyAmount/"/>
		<owl:imports rdf:resource="https://spec.edmcouncil.org/fibo/ontology/FND/Agreements/Contracts/"/>
		<owl:imports rdf:resource="https://spec.edmcouncil.org/fibo/ontology/FND/ArrangementsExt/MethodsAndRules/"/>
		<owl:imports rdf:resource="https://spec.edmcouncil.org/fibo/ontology/FND/DatesAndTimes/FinancialDates/"/>
		<owl:imports rdf:resource="https://spec.edmcouncil.org/fibo/ontology/FND/Parties/Parties/"/>
		<owl:imports rdf:resource="https://spec.edmcouncil.org/fibo/ontology/FND/Relations/Relations/"/>
		<owl:imports rdf:resource="https://spec.edmcouncil.org/fibo/ontology/FND/TransactionsExt/REATransactions/"/>
		<owl:imports rdf:resource="https://spec.edmcouncil.org/fibo/ontology/FND/Utilities/AnnotationVocabulary/"/>
		<owl:versionIRI rdf:resource="https://spec.edmcouncil.org/fibo/ontology/DER/AssetDerivatives/EquityForwards/"/>
		<fibo-fnd-utl-av:hasMaturityLevel rdf:resource="&fibo-fnd-utl-av;Provisional"/>
	</owl:Ontology>
	
	<owl:Class rdf:about="&fibo-der-ass-eqf;CalculationAgentAdjustmentMethod">
		<rdfs:subClassOf rdf:resource="&fibo-der-ass-eqf;ForwardContractAdjustmentMethod"/>
		<rdfs:label xml:lang="en">calculation agent adjustment method</rdfs:label>
		<skos:definition xml:lang="en">The calculation agent has the right to adjust the terms following a corporate event</skos:definition>
	</owl:Class>
	
	<owl:Class rdf:about="&fibo-der-ass-eqf;DividendAdjustmentPeriod">
		<rdfs:subClassOf rdf:resource="&fibo-fnd-dt-fd;DatePeriod"/>
		<rdfs:label xml:lang="en">dividend adjustment period</rdfs:label>
		<skos:definition xml:lang="en">A period used to calculate the Deviation between Expected Dividend and Actual Dividend in that Period.</skos:definition>
		<skos:editorialNote xml:lang="en">Referred to in formal terms for OTC Equity Forwards and Options. REVIEW: It does not look as though we have completely pinned down the meaning on this one, only that it&apos;s a piece of data that&apos;s used for something. We really need to see and model details of those deviation claculations, along with who does them and when. Also they may not directly be facts about the contract as such. REVIEW FpML: &apos;A single Dividend Adjustment Period.&apos;</skos:editorialNote>
	</owl:Class>
	
	<owl:Class rdf:about="&fibo-der-ass-eqf;EquityForwardBuyer">
		<rdfs:subClassOf rdf:resource="&fibo-der-der-fwd;ForwardContractBuyer"/>
		<rdfs:label xml:lang="en">equity forward buyer</rdfs:label>
		<skos:definition xml:lang="en">The party that buys this forwward contract, that is the party which pays for this instrument and receives the rights defined by it.</skos:definition>
		<fibo-fnd-utl-av:explanatoryNote xml:lang="en">See note in Seller. See 2000 ISDA definitions Article 11.1 (b). FpML: &apos;A reference to the party that buys this instrument, ie. pays for this instrument and receives the rights defined by it. See 2000 ISDA definitions Article 11.1 (b). In the case of FRAs this the fixed rate payer.&apos; Interpretation: this is the party which is the counterparty to the contract.</fibo-fnd-utl-av:explanatoryNote>
	</owl:Class>
	
	<owl:Class rdf:about="&fibo-der-ass-eqf;EquityForwardCashSettlement">
		<rdfs:subClassOf rdf:resource="&fibo-der-der-fwd;ForwardCashSettlementTermsSet"/>
		<rdfs:label xml:lang="en">equity forward cash settlement</rdfs:label>
	</owl:Class>
	
	<owl:Class rdf:about="&fibo-der-ass-eqf;EquityForwardContract">
		<rdfs:subClassOf rdf:resource="&fibo-der-ass-ass;EquityDerivativeContract"/>
		<rdfs:subClassOf rdf:resource="&fibo-der-der-fwd;ForwardContract"/>
		<rdfs:subClassOf>
			<owl:Restriction>
				<owl:onProperty rdf:resource="&fibo-der-ass-eqf;dividendAdjustment"/>
				<owl:someValuesFrom rdf:resource="&fibo-der-ass-eqf;DividendAdjustmentPeriod"/>
			</owl:Restriction>
		</rdfs:subClassOf>
		<rdfs:subClassOf>
			<owl:Restriction>
				<owl:onProperty rdf:resource="&fibo-der-ass-eqf;hasConditions"/>
				<owl:someValuesFrom rdf:resource="&fibo-der-ass-eqs;DividendConditions"/>
			</owl:Restriction>
		</rdfs:subClassOf>
		<rdfs:subClassOf>
			<owl:Restriction>
				<owl:onProperty rdf:resource="&fibo-der-ass-eqf;hasMethodOfAdjustment"/>
				<owl:someValuesFrom rdf:resource="&fibo-der-ass-eqf;ForwardContractAdjustmentMethod"/>
			</owl:Restriction>
		</rdfs:subClassOf>
		<rdfs:subClassOf>
			<owl:Restriction>
				<owl:onProperty rdf:resource="https://spec.edmcouncil.org/fibo/ontology/DER/DerivativesContracts/DerivativesBasics/hasUnderlier"/>
				<owl:someValuesFrom rdf:resource="&fibo-der-ass-ass;EquityObservable"/>
			</owl:Restriction>
		</rdfs:subClassOf>
		<rdfs:subClassOf>
			<owl:Restriction>
				<owl:onProperty rdf:resource="&fibo-der-der-fwd;establishes.1"/>
				<owl:someValuesFrom rdf:resource="&fibo-der-ass-eqf;EquityForwardDeliveryCommitment"/>
			</owl:Restriction>
		</rdfs:subClassOf>
		<rdfs:subClassOf>
			<owl:Restriction>
				<owl:onProperty rdf:resource="&fibo-der-der-fwd;hasBuyer"/>
				<owl:someValuesFrom rdf:resource="&fibo-der-ass-eqf;EquityForwardBuyer"/>
			</owl:Restriction>
		</rdfs:subClassOf>
		<rdfs:subClassOf>
			<owl:Restriction>
				<owl:onProperty rdf:resource="&fibo-der-der-fwd;hasSeller"/>
				<owl:someValuesFrom rdf:resource="&fibo-der-ass-eqf;EquityForwardSeller"/>
			</owl:Restriction>
		</rdfs:subClassOf>
		<rdfs:label xml:lang="en">equity forward contract</rdfs:label>
		<skos:definition xml:lang="en">Definition needed</skos:definition>
		<skos:editorialNote xml:lang="en">FpMl definition (unusable): A component describing an Equity Forward product.</skos:editorialNote>
	</owl:Class>
	
	<owl:Class rdf:about="&fibo-der-ass-eqf;EquityForwardDeliveryCommitment">
		<rdfs:subClassOf rdf:resource="&fibo-der-der-fwd;ForwardDeliveryCommitment"/>
		<rdfs:label xml:lang="en">equity forward delivery commitment</rdfs:label>
		<skos:definition xml:lang="en">The commitment to deliver an equity underlying at the maturity of an OTC Equity Forward contract.</skos:definition>
		<skos:editorialNote xml:lang="en">Or, presumably, some cash equivalent in the event that the undelying is non deliverable, or for a non deliverable forward generally.</skos:editorialNote>
	</owl:Class>
	
	<owl:Class rdf:about="&fibo-der-ass-eqf;EquityForwardSeller">
		<rdfs:subClassOf rdf:resource="&fibo-der-der-fwd;ForwardContractSeller"/>
		<rdfs:label xml:lang="en">equity forward seller</rdfs:label>
		<skos:definition xml:lang="en">The party that sells or writes this forward instrument, that is the party which grants the rights defined by this instrument and in return receives a payment for it.</skos:definition>
		<fibo-fnd-utl-av:explanatoryNote xml:lang="en">The forward is always written by the party that is committing to sell the underlying, and is always bought by the party that is committing to take delivery of the underlying on the settlement date. The forward contract is the same as a conventional secondary market sale transaction but with the difference that the settlement date is in the future. See 2000 ISDA definitions Article 11.1 (a). FpML: &apos;A reference to the party that sells (&quot;writes&quot;) this instrument, i.e. that grants the rights defined by this instrument and in return receives a payment for it. See 2000 ISDA definitions Article 11.1 (a). In the case of FRAs this is the floating rate payer.&apos; Interpretation: this is the party which is the principal or writing party to the contract.</fibo-fnd-utl-av:explanatoryNote>
	</owl:Class>
	
	<owl:Class rdf:about="&fibo-der-ass-eqf;EquityForwardTransaction">
		<rdfs:subClassOf rdf:resource="&fibo-der-der-fwd;ForwardTransaction"/>
		<rdfs:subClassOf>
			<owl:Restriction>
				<owl:onProperty rdf:resource="&fibo-der-der-fwd;embodies"/>
				<owl:someValuesFrom rdf:resource="&fibo-der-ass-eqf;EquityForwardContract"/>
			</owl:Restriction>
		</rdfs:subClassOf>
		<rdfs:subClassOf>
			<owl:Restriction>
				<owl:onProperty rdf:resource="&fibo-der-der-fwd;side"/>
				<owl:someValuesFrom rdf:resource="&fibo-der-ass-eqf;EquityForwardCashSettlement"/>
			</owl:Restriction>
		</rdfs:subClassOf>
		<rdfs:subClassOf>
			<owl:Restriction>
				<owl:onProperty rdf:resource="&fibo-der-der-fwd;side.1"/>
				<owl:someValuesFrom rdf:resource="&fibo-der-ass-ass;SecurityForwardDelivery"/>
			</owl:Restriction>
		</rdfs:subClassOf>
		<rdfs:label xml:lang="en">equity forward transaction</rdfs:label>
		<skos:definition xml:lang="en">A transaction in which one party commits at the present to delivery of an equity security or securities or cash equivalent in the future.</skos:definition>
	</owl:Class>
	
	<owl:Class rdf:about="&fibo-der-ass-eqf;EquitySecurityDelivery">
		<rdfs:subClassOf rdf:resource="&fibo-der-ass-ass;UnderlyingSecurityDelivery"/>
		<rdfs:label xml:lang="en">equity security delivery</rdfs:label>
	</owl:Class>
	
	<owl:Class rdf:about="&fibo-der-ass-eqf;EquityValuation">
		<rdfs:subClassOf rdf:resource="&fibo-der-der-fwd;UnderlyingValuation"/>
		<rdfs:subClassOf>
			<owl:Restriction>
				<owl:onProperty rdf:resource="&fibo-der-der-fwd;undertakenBy"/>
				<owl:someValuesFrom rdf:resource="&fibo-der-ass-eqf;EquityValuationCalculationAgent"/>
			</owl:Restriction>
		</rdfs:subClassOf>
		<rdfs:label xml:lang="en">equity valuation</rdfs:label>
		<skos:definition xml:lang="en">The act of valuation of an equity underlying (share, basket or index) during the life of an OTC equity option or forward.</skos:definition>
		<fibo-fnd-utl-av:explanatoryNote xml:lang="en">FpML: &apos;The parameters for defining when valuation of the underlying takes place.&apos;</fibo-fnd-utl-av:explanatoryNote>
	</owl:Class>
	
	<owl:Class rdf:about="&fibo-der-ass-eqf;EquityValuationCalculationAgent">
		<rdfs:subClassOf rdf:resource="&fibo-der-der-fwd;CalculationAgent"/>
		<rdfs:label xml:lang="en">equity valuation calculation agent</rdfs:label>
		<skos:definition xml:lang="en">The entity which carries out the valuation of an asset underlying an equity forward or option, or from which the valuation of the underlying is to be taken.</skos:definition>
	</owl:Class>
	
	<owl:Class rdf:about="&fibo-der-ass-eqf;ForwardContractAdjustmentMethod">
		<rdfs:subClassOf rdf:resource="&fibo-fnd-arrxx-meth;AdjustmentMethod"/>
		<rdfs:label xml:lang="en">forward contract adjustment method</rdfs:label>
		<skos:definition xml:lang="en">Method by which adjustments will be made to the forward contract should one or more of a number of extraordinary events occur.</skos:definition>
		<fibo-fnd-utl-av:explanatoryNote xml:lang="en">FpML: Defines how adjustments will be made to the contract should one or more of the extraordinary events occur.</fibo-fnd-utl-av:explanatoryNote>
	</owl:Class>
	
	<owl:Class rdf:about="&fibo-der-ass-eqf;OptionsExchangeAdjustmentMethod">
		<rdfs:subClassOf rdf:resource="&fibo-der-ass-eqf;ForwardContractAdjustmentMethod"/>
		<rdfs:label xml:lang="en">options exchange adjustment method</rdfs:label>
		<skos:definition xml:lang="en">The trade will be adjusted according to ... exchange on which the options (??) are listed</skos:definition>
		<skos:editorialNote xml:lang="en">REVIEW: Seems to be traded-option-underlying specific.</skos:editorialNote>
	</owl:Class>
	
	<owl:ObjectProperty rdf:about="&fibo-der-ass-eqf;dividendAdjustment">
		<rdfs:label xml:lang="en">dividend adjustment</rdfs:label>
		<rdfs:domain rdf:resource="&fibo-der-ass-eqf;EquityForwardContract"/>
		<rdfs:range rdf:resource="&fibo-der-ass-eqf;DividendAdjustmentPeriod"/>
		<skos:definition xml:lang="en">One or more Dividend Adjustment Periods, which are used to calculate the Deviation between Expected Dividend and Actual Dividend in that Period.&apos;</skos:definition>
	</owl:ObjectProperty>
	
	<owl:ObjectProperty rdf:about="&fibo-der-ass-eqf;hasConditions">
		<rdfs:label xml:lang="en">has conditions</rdfs:label>
		<rdfs:domain rdf:resource="&fibo-der-ass-eqf;EquityForwardContract"/>
		<rdfs:range rdf:resource="&fibo-der-ass-eqs;DividendConditions"/>
	</owl:ObjectProperty>
	
	<owl:ObjectProperty rdf:about="&fibo-der-ass-eqf;hasMethodOfAdjustment">
		<rdfs:label xml:lang="en">has method of adjustment</rdfs:label>
		<rdfs:domain rdf:resource="&fibo-der-ass-eqf;EquityForwardContract"/>
		<rdfs:range rdf:resource="&fibo-der-ass-eqf;ForwardContractAdjustmentMethod"/>
	</owl:ObjectProperty>
	
	<owl:DatatypeProperty rdf:about="&fibo-der-ass-eqf;priceSource">
		<rdfs:label xml:lang="en">price source</rdfs:label>
		<rdfs:domain rdf:resource="&fibo-der-ass-eqf;EquityForwardCashSettlement"/>
		<rdfs:range rdf:resource="&xsd;string"/>
		<skos:definition xml:lang="en">The Price source to be used to determine the settlement price.</skos:definition>
	</owl:DatatypeProperty>
	
	<owl:DatatypeProperty rdf:about="&fibo-der-ass-eqf;settlementMethodElection">
		<rdfs:label xml:lang="en">settlement method election</rdfs:label>
		<rdfs:domain rdf:resource="&fibo-der-ass-eqf;EquityForwardCashSettlement"/>
		<rdfs:range rdf:resource="&xsd;string"/>
		<skos:definition xml:lang="en">How the forward will be settled.</skos:definition>
	</owl:DatatypeProperty>

</rdf:RDF>