<?xml version="1.0" encoding="UTF-8"?>

<!DOCTYPE rdf:RDF [
    <!ENTITY rdf "http://www.w3.org/1999/02/22-rdf-syntax-ns#" >
    <!ENTITY rdfs "http://www.w3.org/2000/01/rdf-schema#" >
    <!ENTITY owl "http://www.w3.org/2002/07/owl#" >
    <!ENTITY xsd "http://www.w3.org/2001/XMLSchema#" >
    <!ENTITY dct "http://purl.org/dc/terms/" >
    <!ENTITY skos "http://www.w3.org/2004/02/skos/core#" >
    <!ENTITY sm "http://www.omg.org/techprocess/ab/SpecificationMetadata/" >
    <!ENTITY fibo-fnd-utl-av "http://www.omg.org/spec/EDMC-FIBO/FND/Utilities/AnnotationVocabulary/" >
    <!ENTITY fibo-fnd-utl-bt "http://www.omg.org/spec/EDMC-FIBO/FND/Utilities/BusinessFacingTypes/" >
    <!ENTITY fibo-fnd-rel-rel "http://www.omg.org/spec/EDMC-FIBO/FND/Relations/Relations/" >
    <!ENTITY fibo-fnd-aap-agt "http://www.omg.org/spec/EDMC-FIBO/FND/AgentsAndPeople/Agents/" >
    <!ENTITY fibo-fnd-plc-loc "http://www.omg.org/spec/EDMC-FIBO/FND/Places/Locations/" >
    <!ENTITY fibo-fnd-plc-cty "http://www.omg.org/spec/EDMC-FIBO/FND/Places/Countries/" >
    <!ENTITY fibo-fnd-plc-adr "http://www.omg.org/spec/EDMC-FIBO/FND/Places/Addresses/" >
    <!ENTITY fibo-fnd-gao-gl "http://www.omg.org/spec/EDMC-FIBO/FND/GoalsAndObjectives/Goals/" >
    <!ENTITY fibo-fnd-org-org "http://www.omg.org/spec/EDMC-FIBO/FND/Organizations/Organizations/" >
    <!ENTITY fibo-fnd-org-fm "http://www.omg.org/spec/EDMC-FIBO/FND/Organizations/FormalOrganizations/" >
    <!ENTITY fibo-fnd-law-cor "http://www.omg.org/spec/EDMC-FIBO/FND/Law/LegalCore/" >
    <!ENTITY fibo-fnd-law-jur "http://www.omg.org/spec/EDMC-FIBO/FND/Law/Jurisdiction/" >
]>

<rdf:RDF xmlns="http://www.omg.org/spec/EDMC-FIBO/FND/Law/Jurisdiction/"
xml:base="http://www.omg.org/spec/EDMC-FIBO/FND/Law/Jurisdiction/"
     xmlns:rdf="http://www.w3.org/1999/02/22-rdf-syntax-ns#"
     xmlns:rdfs="http://www.w3.org/2000/01/rdf-schema#"
     xmlns:owl="http://www.w3.org/2002/07/owl#"
     xmlns:xsd="http://www.w3.org/2001/XMLSchema#"
     xmlns:dct="http://purl.org/dc/terms/"
     xmlns:skos="http://www.w3.org/2004/02/skos/core#"
xmlns:sm="http://www.omg.org/techprocess/ab/SpecificationMetadata/"
     xmlns:fibo-fnd-utl-av="http://www.omg.org/spec/EDMC-FIBO/FND/Utilities/AnnotationVocabulary/"
     xmlns:fibo-fnd-utl-bt="http://www.omg.org/spec/EDMC-FIBO/FND/Utilities/BusinessFacingTypes/"
     xmlns:fibo-fnd-rel-rel="http://www.omg.org/spec/EDMC-FIBO/FND/Relations/Relations/"
     xmlns:fibo-fnd-aap-agt="http://www.omg.org/spec/EDMC-FIBO/FND/AgentsAndPeople/Agents/"
     xmlns:fibo-fnd-gao-gl="http://www.omg.org/spec/EDMC-FIBO/FND/GoalsAndObjectives/Goals/"
     xmlns:fibo-fnd-plc-loc="http://www.omg.org/spec/EDMC-FIBO/FND/Places/Locations/"
     xmlns:fibo-fnd-plc-cty="http://www.omg.org/spec/EDMC-FIBO/FND/Places/Countries/"
     xmlns:fibo-fnd-plc-adr="http://www.omg.org/spec/EDMC-FIBO/FND/Places/Addresses/"
     xmlns:fibo-fnd-org-org="http://www.omg.org/spec/EDMC-FIBO/FND/Organizations/Organizations/"
     xmlns:fibo-fnd-org-fm="http://www.omg.org/spec/EDMC-FIBO/FND/Organizations/FormalOrganizations/"
     xmlns:fibo-fnd-law-cor="http://www.omg.org/spec/EDMC-FIBO/FND/Law/LegalCore/"
     xmlns:fibo-fnd-law-jur="http://www.omg.org/spec/EDMC-FIBO/FND/Law/Jurisdiction/">
         

    <owl:Ontology rdf:about="http://www.omg.org/spec/EDMC-FIBO/FND/Law/Jurisdiction/">
        <rdfs:label>Financial Industry Business Ontology (FIBO) Jurisdiction Ontology</rdfs:label>


    <!-- Specification Family Level Metadata for the FIBO Formal Organizations Ontology -->

        <sm:familyTitle rdf:datatype="&xsd;string">Financial Industry Business Ontology (FIBO)</sm:familyTitle>
        <sm:familyAbbreviation rdf:datatype="&xsd;string">FIBO</sm:familyAbbreviation>
        <sm:familyURL rdf:datatype="&xsd;anyURI">http://www.omg.org/spec/EDMC-FIBO/</sm:familyURL>
        <sm:familyAbstract rdf:datatype="&xsd;string">The content that comprises the Financial Industry Business Ontology (FIBO) is documentation, interpretable in formal logic, of the concepts represented by finance industry terms as used in official financial organization documents such as contracts, product/service specifications and governance and regulatory compliance documents.</sm:familyAbstract>

        <sm:technologyArea rdf:datatype="&xsd;string">formal semantics</sm:technologyArea>

        <sm:topicArea rdf:datatype="&xsd;string">finance</sm:topicArea>

        <sm:keyword rdf:datatype="&xsd;string">Financial Industry Business Ontology</sm:keyword>
        <sm:keyword rdf:datatype="&xsd;string">FIBO</sm:keyword>
        <sm:keyword rdf:datatype="&xsd;string">ontology</sm:keyword>
        <sm:keyword rdf:datatype="&xsd;string">vocabulary</sm:keyword>


    <!-- Specification Level Metadata for the FIBO Jurisdiction Ontology -->

        <sm:specificationTitle rdf:datatype="&xsd;string">Financial Industry Business Ontology (FIBO) Foundations Specification</sm:specificationTitle>
        <sm:specificationAbbreviation rdf:datatype="&xsd;string">FIBO-FND</sm:specificationAbbreviation>
        <sm:specificationURL rdf:datatype="&xsd;anyURI">http://www.omg.org/spec/EDMC-FIBO/FND/</sm:specificationURL>
        <sm:specificationAbstract rdf:datatype="&xsd;string">FIBO Foundations is a set of business concepts which are intended to support the financial industry terms semantics presented in other FIBO specifications.  

The FIBO Foundations models define concepts which are not unique to the financial services industry. From these, financial industry terms in other FIBO specifications may be derived by extension. Terms are also included which may be referred to by properties of things in those specifications. FIBO Foundations therefore includes a number of basic terms about legal, contractual and organizational concepts, among others. </sm:specificationAbstract>

        <sm:dependsOn rdf:datatype="&xsd;anyURI">http://www.omg.org/techprocess/ab/SpecificationMetadata/</sm:dependsOn>

        <sm:keyword rdf:datatype="&xsd;string">foundational vocabulary</sm:keyword>


    <!-- Specification Version Metadata for the FIBO Jurisdiction Ontology -->

        <sm:thisVersion rdf:datatype="&xsd;string">1.0 </sm:thisVersion>
        <sm:publicationDate rdf:datatype="&xsd;dateTime">2013-08-26T18:00:00</sm:publicationDate>
        <sm:specificationVersionURL rdf:datatype="&xsd;anyURI">http://www.omg.org/spec/EDMC-FIBO/FND/1.0/</sm:specificationVersionURL>
        <sm:specificationVersionStatus rdf:datatype="&xsd;string">Request For Comments (RFC)</sm:specificationVersionStatus>
        <skos:historyNote rdf:datatype="&xsd;string">This version of the FIBO Foundations Specification was revised primarily to reflect comments received at the March 2013 OMG Technical Meeting in Reston and reflected in the Errata discussed at the June 2013 OMG Technical Meeting in Berlin. 

Revisions to FIBO Foundations are managed per the process outlined in the Policies and Procedures for OMG standards, with the intent to maintain backwards compatibility in the ontologies to the degree possible.
  
The RDF/XML serialized OWL for the Foundations ODM/OWL ontologies have been checked for syntactic errors and logical consistency with Protege 4 (http://protege.stanford.edu/), HermiT 1.3.7 (http://www.hermit-reasoner.com/) and Pellet 2.2 (http://clarkparsia.com/pellet/).</skos:historyNote>
        <sm:addressForComments rdf:datatype="&xsd;anyURI">http://www.omg.org/issues/</sm:addressForComments>


    <!-- Module Level Metadata for the FIBO Jurisdiction Ontology -->

        <sm:moduleName rdf:datatype="&xsd;string">Law</sm:moduleName>
        <sm:moduleAbbreviation rdf:datatype="&xsd;string">FIBO-FND-LAW</sm:moduleAbbreviation>
        <sm:moduleVersion rdf:datatype="&xsd;string">1.0</sm:moduleVersion>
        <sm:moduleAbstract rdf:datatype="&xsd;string">This module includes several ontologies defining legal concepts, including constitutions, laws and jurisdictions. It also includes the definition of legal capacities such as signatory capacity, contractual capability and the like.</sm:moduleAbstract>


    <!-- Curation and Rights Metadata for the FIBO Jurisdiction Ontology -->

        <sm:copyright rdf:datatype="&xsd;string">Copyright (c) 2013 EDM Council, Inc.
Copyright (c) 2013 Object Management Group, Inc.</sm:copyright>
        <sm:submitter rdf:datatype="&xsd;string">EDM Council, Inc.</sm:submitter>
        <sm:contributor rdf:datatype="&xsd;string">Adaptive, Inc.</sm:contributor>
        <sm:contributor rdf:datatype="&xsd;string">Thematix Partners LLC</sm:contributor>
        <dct:license rdf:datatype="&xsd;string">The MIT License:  Permission is hereby granted, free of charge, to any person obtaining a copy of this software and associated documentation files (the &quot;Software&quot;), to deal in the Software without restriction, including without limitation the rights to use, copy, modify, merge, publish, distribute, sublicense, and/or sell copies of the Software, and to permit persons to whom the Software is furnished to do so, subject to the following conditions:

The copyright notice and this permission notice shall be included in all copies or substantial portions of the Software.

THE SOFTWARE IS PROVIDED &quot;AS IS&quot;, WITHOUT WARRANTY OF ANY KIND, EXPRESS OR IMPLIED, INCLUDING BUT NOT LIMITED TO THE WARRANTIES OF MERCHANTABILITY, FITNESS FOR A PARTICULAR PURPOSE
AND NONINFRINGEMENT.  IN NO EVENT SHALL THE AUTHORS OR COPYRIGHT HOLDERS BE LIABLE FOR ANY CLAIM, DAMAGES OR OTHER LIABILITY, WHETHER IN AN ACTION OF CONTRACT, TORT OR OTHERWISE, ARISING FROM, OUT OF OR IN CONNECTION WITH THE SOFTWARE OR THE USE OR OTHER DEALINGS IN THE SOFTWARE.</dct:license>
        <dct:license rdf:datatype="&xsd;anyURI">http://opensource.org/licenses/mit-license.php</dct:license>
        <sm:responsibleTaskForce rdf:datatype="&xsd;anyURI">http://fdtf.omg.org/</sm:responsibleTaskForce>


    <!-- Ontology/File-Level Metadata for the Jurisdiction Ontology -->

        <sm:filename rdf:datatype="&xsd;string">Jurisdiction.owl</sm:filename>
        <sm:fileAbbreviation rdf:datatype="&xsd;string">fibo-fnd-law-jur</sm:fileAbbreviation>
        <owl:versionIRI rdf:datatype="&xsd;anyURI">http://www.omg.org/spec/EDMC-FIBO/FND/20130801/Law/Jurisdiction/</owl:versionIRI>
        <sm:priorVersion rdf:datatype="&xsd;anyURI">http://www.omg.org/spec/FIBO/Foundations/20130601/Law/Jurisdiction.owl</sm:priorVersion>
        <sm:fileAbstract rdf:datatype="&xsd;string">This ontology defines high level concepts relating to jurisdictions for use in other FIBO ontology elements. This includes a general definition of jurisdiction along with some basic types of jurisdiction, along with the factors which distinguish one type of jurisdiction from another. This ontology also defines basic types of legal system, and extends the basic concept of law which is in the LegalCore ontology..</sm:fileAbstract>
        <skos:changeNote rdf:datatype="&xsd;string">This version of the ontology was revised in advance of the September 2013 New Brunswick, NJ meeting, as follows:
   (1) to use slash style URI/IRIss (also called 303 URIs, vs. hash style) as required to support server side processing 
   (2) to use version-independent IRIs for all definitions internally as opposed to version-specific IRIs
   (3) to change the file suffix from .owl to .rdf to increase usability in RDF tools
   (4) to use 4-level abbreviations and corresponding namespace prefixes for all FIBO ontologies, reflecting a family/specification/module/ontology structure
   (5) to incorporate changes to the specification metadata to support documentation at the family, specification, module, and ontology level, similar to the abbreviations
   (6) to revise definitions using more formal sources.</skos:changeNote>

        <sm:dependsOn rdf:datatype="&xsd;anyURI">http://www.omg.org/spec/EDMC-FIBO/FND/Utilities/AnnotationVocabulary/</sm:dependsOn>
        <sm:dependsOn rdf:datatype="&xsd;anyURI">http://www.omg.org/spec/EDMC-FIBO/FND/Utilities/BusinessFacingTypes/</sm:dependsOn>
        <sm:dependsOn rdf:datatype="&xsd;anyURI">http://www.omg.org/spec/EDMC-FIBO/FND/Relations/Relations/</sm:dependsOn>
        <sm:dependsOn rdf:datatype="&xsd;anyURI">http://www.omg.org/spec/EDMC-FIBO/FND/AgentsAndPeople/Agents/</sm:dependsOn>
        <sm:dependsOn rdf:datatype="&xsd;anyURI">http://www.omg.org/spec/EDMC-FIBO/FND/GoalsAndObjectives/Goals/</sm:dependsOn>
        <sm:dependsOn rdf:datatype="&xsd;anyURI">http://www.omg.org/spec/EDMC-FIBO/FND/Places/Locations/</sm:dependsOn>
        <sm:dependsOn rdf:datatype="&xsd;anyURI">http://www.omg.org/spec/EDMC-FIBO/FND/Places/Countries/</sm:dependsOn>
        <sm:dependsOn rdf:datatype="&xsd;anyURI">http://www.omg.org/spec/EDMC-FIBO/FND/Places/Addresses/</sm:dependsOn>
        <sm:dependsOn rdf:datatype="&xsd;anyURI">http://www.omg.org/spec/EDMC-FIBO/FND/Organizations/Organizations/</sm:dependsOn>
        <sm:dependsOn rdf:datatype="&xsd;anyURI">http://www.omg.org/spec/EDMC-FIBO/FND/Organizations/FormalOrganizations/</sm:dependsOn>
        <sm:dependsOn rdf:datatype="&xsd;anyURI">http://www.omg.org/spec/EDMC-FIBO/FND/Law/LegalCore/</sm:dependsOn>


        <sm:contentLanguage rdf:datatype="&xsd;anyURI">http://www.w3.org/standards/techs/owl#w3c_all</sm:contentLanguage>
        <sm:contentLanguage rdf:datatype="&xsd;anyURI">http://www.omg.org/spec/ODM/</sm:contentLanguage>


        <owl:imports rdf:resource="http://www.omg.org/techprocess/ab/SpecificationMetadata/"/>
        <owl:imports rdf:resource="http://www.omg.org/spec/EDMC-FIBO/FND/Utilities/AnnotationVocabulary/"/>
        <owl:imports rdf:resource="http://www.omg.org/spec/EDMC-FIBO/FND/Utilities/BusinessFacingTypes/"/>
        <owl:imports rdf:resource="http://www.omg.org/spec/EDMC-FIBO/FND/Relations/Relations/"/>
        <owl:imports rdf:resource="http://www.omg.org/spec/EDMC-FIBO/FND/AgentsAndPeople/Agents/"/>
        <owl:imports rdf:resource="http://www.omg.org/spec/EDMC-FIBO/FND/GoalsAndObjectives/Goals/"/>
        <owl:imports rdf:resource="http://www.omg.org/spec/EDMC-FIBO/FND/Places/Locations/"/>
        <owl:imports rdf:resource="http://www.omg.org/spec/EDMC-FIBO/FND/Places/Countries/"/>
        <owl:imports rdf:resource="http://www.omg.org/spec/EDMC-FIBO/FND/Places/Addresses/"/>
        <owl:imports rdf:resource="http://www.omg.org/spec/EDMC-FIBO/FND/Organizations/Organizations/"/>
        <owl:imports rdf:resource="http://www.omg.org/spec/EDMC-FIBO/FND/Organizations/FormalOrganizations/"/>
        <owl:imports rdf:resource="http://www.omg.org/spec/EDMC-FIBO/FND/Law/LegalCore/"/>
   </owl:Ontology>


    <!-- 
    ///////////////////////////////////////////////////////////////////////////////////////
    //
    // Object Properties
    //
    ///////////////////////////////////////////////////////////////////////////////////////
     -->

    <owl:ObjectProperty rdf:about="&fibo-fnd-law-jur;appliesIn">
        <rdfs:label>applies in</rdfs:label>
        <skos:definition>indicates the jurisdiction in which a particular legal system applies</skos:definition>
        <rdfs:subPropertyOf rdf:resource="&fibo-fnd-rel-rel;governs"/>
    </owl:ObjectProperty>

    <owl:ObjectProperty rdf:about="&fibo-fnd-law-jur;hasReach">
        <rdfs:label>has reach</rdfs:label>
        <skos:definition>indicates the geopolitical entity (country, federal province or municipality) in which the jurisdiction has effect</skos:definition>
        <rdfs:domain rdf:resource="&fibo-fnd-law-jur;Jurisdiction"/>
        <rdfs:range rdf:resource="&fibo-fnd-plc-cty;GeopoliticalEntity"/>
    </owl:ObjectProperty>


    <!-- 
    ///////////////////////////////////////////////////////////////////////////////////////
    //
    // Classes
    //
    ///////////////////////////////////////////////////////////////////////////////////////
     -->

    <owl:Class rdf:about="&fibo-fnd-law-jur;CivilLawJurisdiction">
        <rdfs:label>civil law jurisdiction</rdfs:label>
        <rdfs:subClassOf rdf:resource="&fibo-fnd-law-jur;Jurisdiction"/>
        <rdfs:subClassOf>
             <owl:Restriction>
                 <owl:onProperty rdf:resource="&fibo-fnd-rel-rel;isGovernedBy"/>
                 <owl:allValuesFrom rdf:resource="&fibo-fnd-law-jur;CivilLawSystem"/>
             </owl:Restriction>
        </rdfs:subClassOf>
        <skos:definition>a civil law jurisdiction</skos:definition>
    </owl:Class>

    <owl:Class rdf:about="&fibo-fnd-law-jur;CivilLawSystem">
        <rdfs:label>civil law system</rdfs:label>
        <rdfs:subClassOf>
             <owl:Restriction>
                 <owl:onProperty rdf:resource="&fibo-fnd-law-jur;appliesIn"/>
                 <owl:someValuesFrom rdf:resource="&fibo-fnd-law-jur;CivilLawJurisdiction"/>
             </owl:Restriction>
        </rdfs:subClassOf>
        <skos:definition>Civil law (or civilian law) is a legal system originating in Europe, intellectualized within the framework of late Roman law, and whose most prevalent feature is that its core principles are codified into a referable system which serves as the primary source of law.  This can be contrasted with common law systems whose intellectual framework comes from judge-made decisional law which gives precedential authority to prior court decisions on the principle that it is unfair to treat similar facts differently on different occasions (doctrine of judicial precedent).</skos:definition>
        <fibo-fnd-utl-av:definitionOrigin>http://en.wikipedia.org/wiki/Civil_law_(legal_system)</fibo-fnd-utl-av:definitionOrigin>
        <rdfs:subClassOf rdf:resource="&fibo-fnd-law-jur;LegalSystem"/>
    </owl:Class>

    <owl:Class rdf:about="&fibo-fnd-law-jur;CommonLawJurisdiction">
        <rdfs:label>common law jurisdiction</rdfs:label>
        <rdfs:subClassOf rdf:resource="&fibo-fnd-law-jur;Jurisdiction"/>
        <rdfs:subClassOf>
             <owl:Restriction>
                 <owl:onProperty rdf:resource="&fibo-fnd-rel-rel;isGovernedBy"/>
                 <owl:allValuesFrom rdf:resource="&fibo-fnd-law-jur;CommonLawSystem"/>
             </owl:Restriction>
        </rdfs:subClassOf>
        <skos:definition>a jurisdiction based on common law</skos:definition>
    </owl:Class>

    <owl:Class rdf:about="&fibo-fnd-law-jur;CommonLawSystem">
        <rdfs:label>common law system</rdfs:label>
        <rdfs:subClassOf rdf:resource="&fibo-fnd-law-jur;LegalSystem"/>
        <rdfs:subClassOf>
             <owl:Restriction>
                 <owl:onProperty rdf:resource="&fibo-fnd-law-jur;appliesIn"/>
                 <owl:someValuesFrom rdf:resource="&fibo-fnd-law-jur;CommonLawJurisdiction"/>
             </owl:Restriction>
        </rdfs:subClassOf>
        <skos:definition>Common law, also known as case law or precedent, is law developed by judges through decisions of courts and similar tribunals.  By contrast, civil law (codified/continental law) is set on statutes adopted through the legislative/parliamentary process and/or regulations issued by the executive branch on base of the parliamentary statutes.

A common law system is a legal system that gives great potential precedential weight to common law, on the principle that it is unfair to treat similar facts differently on different occasions. The body of precedent is called common law and it binds future decisions. In cases where the parties disagree on what the law is, a common law court looks to past precedential decisions of relevant courts. If a similar dispute has been resolved in the past, the court is bound to follow the reasoning used in the prior decision (this principle is known as stare decisis). If, however, the court finds that the current dispute is fundamentally distinct from all previous cases (called a matter of first impression), judges have the authority and duty to make law by creating precedent. Thereafter, the new decision becomes precedent, and will bind future courts.</skos:definition>
        <fibo-fnd-utl-av:definitionOrigin>http://en.wikipedia.org/wiki/Common_law</fibo-fnd-utl-av:definitionOrigin>
        <skos:editorialNote>A jurisdiction which is based in Common Law will also have alongside a legislature that passes statutes.</skos:editorialNote>
    </owl:Class>

    <owl:Class rdf:about="&fibo-fnd-law-jur;Jurisdiction">
        <rdfs:label>jurisdiction</rdfs:label>
        <skos:definition>the limits or territory within which authority may be exercised; the power, right, or authority to interpret and apply the law</skos:definition>
        <fibo-fnd-utl-av:definitionOrigin>Merriam-Webster Online Dictionary</fibo-fnd-utl-av:definitionOrigin>
        <rdfs:subClassOf>
             <owl:Restriction>
                 <owl:onProperty rdf:resource="&fibo-fnd-rel-rel;isGovernedBy"/>
                 <owl:allValuesFrom rdf:resource="&fibo-fnd-law-jur;LegalSystem"/>
             </owl:Restriction>
        </rdfs:subClassOf>
        <rdfs:subClassOf>
             <owl:Restriction>
                 <owl:onProperty rdf:resource="&fibo-fnd-law-jur;hasReach"/>
                 <owl:someValuesFrom rdf:resource="&fibo-fnd-plc-cty;GeopoliticalEntity"/>
             </owl:Restriction>
        </rdfs:subClassOf>
    </owl:Class>

    <owl:Class rdf:about="&fibo-fnd-law-jur;LegalSystem">
        <rdfs:label>legal system</rdfs:label>
        <skos:definition>The contemporary legal systems of the world are generally based on one of three basic systems: civil law, common law, and religious law, or combinations of these. However, the legal system of each country is shaped by its unique history and so incorporates individual variations.</skos:definition>
        <fibo-fnd-utl-av:definitionOrigin>http://en.wikipedia.org/wiki/Legal_systems_of_the_world</fibo-fnd-utl-av:definitionOrigin>
        <skos:editorialNote>This is a Mediating Thing, that is some context in which things have their meaning and existence - in this case, laws and the interpretation thereof by courts.</skos:editorialNote>
        <rdfs:subClassOf>
             <owl:Restriction>
                 <owl:onProperty rdf:resource="&fibo-fnd-rel-rel;isGovernedBy"/>
                 <owl:allValuesFrom rdf:resource="&fibo-fnd-law-cor;GovernmentalConstitution"/>
             </owl:Restriction>
        </rdfs:subClassOf>
        <rdfs:subClassOf>
             <owl:Restriction>
                 <owl:onProperty rdf:resource="&fibo-fnd-law-jur;appliesIn"/>
                 <owl:allValuesFrom rdf:resource="&fibo-fnd-law-jur;Jurisdiction"/>
             </owl:Restriction>
        </rdfs:subClassOf>
        <skos:definition>a system of law</skos:definition>
   </owl:Class>

    <owl:Class rdf:about="&fibo-fnd-law-jur;StatuteLaw">
        <rdfs:label>statute law</rdfs:label>
        <skos:altLabel>statutory law</skos:altLabel>
        <rdfs:subClassOf>
             <owl:Restriction>
                 <owl:onProperty rdf:resource="&fibo-fnd-rel-rel;isInForceIn"/>
                 <owl:allValuesFrom rdf:resource="&fibo-fnd-law-jur;Jurisdiction"/>
             </owl:Restriction>
        </rdfs:subClassOf>
        <skos:definition>Statutory law or statute law is written law (as opposed to oral or customary law) set down by a legislature (as opposed to regulatory law promulgated by the executive or common law of the judiciary) or by a legislator (in the case of an absolute monarchy). Statutes may originate with national, state legislatures or local municipalities. Statutory laws are subordinate to the higher constitutional laws of the land.</skos:definition>
        <fibo-fnd-utl-av:definitionOrigin>http://en.wikipedia.org/wiki/Statute_law</fibo-fnd-utl-av:definitionOrigin>
        <rdfs:subClassOf rdf:resource="&fibo-fnd-law-cor;Law"/>
   </owl:Class>

</rdf:RDF>