<?xml version="1.0" encoding="UTF-8"?>

<!DOCTYPE rdf:RDF [
    <!ENTITY rdf "http://www.w3.org/1999/02/22-rdf-syntax-ns#" >
    <!ENTITY rdfs "http://www.w3.org/2000/01/rdf-schema#" >
    <!ENTITY owl "http://www.w3.org/2002/07/owl#" >
    <!ENTITY xsd "http://www.w3.org/2001/XMLSchema#" >
    <!ENTITY dct "http://purl.org/dc/terms/" >
    <!ENTITY skos "http://www.w3.org/2004/02/skos/core#" >
    <!ENTITY sm "http://www.omg.org/techprocess/ab/SpecificationMetadata/" >
    <!ENTITY fibo-fnd-utl-av "http://www.omg.org/spec/EDMC-FIBO/FND/Utilities/AnnotationVocabulary/" >
    <!ENTITY fibo-fnd-utl-bt "http://www.omg.org/spec/EDMC-FIBO/FND/Utilities/BusinessFacingTypes/" >
    <!ENTITY fibo-fnd-rel-rel "http://www.omg.org/spec/EDMC-FIBO/FND/Relations/Relations/" >
    <!ENTITY fibo-fnd-aap-agt "http://www.omg.org/spec/EDMC-FIBO/FND/AgentsAndPeople/Agents/" >
    <!ENTITY fibo-fnd-plc-loc "http://www.omg.org/spec/EDMC-FIBO/FND/Places/Locations/" >
    <!ENTITY fibo-fnd-plc-cty "http://www.omg.org/spec/EDMC-FIBO/FND/Places/Countries/" >
    <!ENTITY fibo-fnd-plc-adr "http://www.omg.org/spec/EDMC-FIBO/FND/Places/Addresses/" >
    <!ENTITY fibo-fnd-gao-gl "http://www.omg.org/spec/EDMC-FIBO/FND/GoalsAndObjectives/Goals/" >
    <!ENTITY fibo-fnd-org-org "http://www.omg.org/spec/EDMC-FIBO/FND/Organizations/Organizations/" >
    <!ENTITY fibo-fnd-org-fm "http://www.omg.org/spec/EDMC-FIBO/FND/Organizations/FormalOrganizations/" >
    <!ENTITY fibo-fnd-law-cor "http://www.omg.org/spec/EDMC-FIBO/FND/Law/LegalCore/" >
]>

<rdf:RDF xmlns="http://www.omg.org/spec/EDMC-FIBO/FND/Law/LegalCore/"
xml:base="http://www.omg.org/spec/EDMC-FIBO/FND/Law/LegalCore/"
     xmlns:rdf="http://www.w3.org/1999/02/22-rdf-syntax-ns#"
     xmlns:rdfs="http://www.w3.org/2000/01/rdf-schema#"
     xmlns:owl="http://www.w3.org/2002/07/owl#"
     xmlns:xsd="http://www.w3.org/2001/XMLSchema#"
     xmlns:dct="http://purl.org/dc/terms/"
     xmlns:skos="http://www.w3.org/2004/02/skos/core#"
xmlns:sm="http://www.omg.org/techprocess/ab/SpecificationMetadata/"
     xmlns:fibo-fnd-utl-av="http://www.omg.org/spec/EDMC-FIBO/FND/Utilities/AnnotationVocabulary/"
     xmlns:fibo-fnd-utl-bt="http://www.omg.org/spec/EDMC-FIBO/FND/Utilities/BusinessFacingTypes/"
     xmlns:fibo-fnd-rel-rel="http://www.omg.org/spec/EDMC-FIBO/FND/Relations/Relations/"
     xmlns:fibo-fnd-aap-agt="http://www.omg.org/spec/EDMC-FIBO/FND/AgentsAndPeople/Agents/"
     xmlns:fibo-fnd-gao-gl="http://www.omg.org/spec/EDMC-FIBO/FND/GoalsAndObjectives/Goals/"
     xmlns:fibo-fnd-plc-loc="http://www.omg.org/spec/EDMC-FIBO/FND/Places/Locations/"
     xmlns:fibo-fnd-plc-cty="http://www.omg.org/spec/EDMC-FIBO/FND/Places/Countries/"
     xmlns:fibo-fnd-plc-adr="http://www.omg.org/spec/EDMC-FIBO/FND/Places/Addresses/"
     xmlns:fibo-fnd-org-org="http://www.omg.org/spec/EDMC-FIBO/FND/Organizations/Organizations/"
     xmlns:fibo-fnd-org-fm="http://www.omg.org/spec/EDMC-FIBO/FND/Organizations/FormalOrganizations/"
     xmlns:fibo-fnd-law-cor="http://www.omg.org/spec/EDMC-FIBO/FND/Law/LegalCore/">


    <owl:Ontology rdf:about="http://www.omg.org/spec/EDMC-FIBO/FND/Law/LegalCore/">
        <rdfs:label>Financial Industry Business Ontology (FIBO) Legal Core Ontology</rdfs:label>


    <!-- Specification Family Level Metadata for the FIBO Formal Organizations Ontology -->

        <sm:familyTitle rdf:datatype="&xsd;string">Financial Industry Business Ontology (FIBO)</sm:familyTitle>
        <sm:familyAbbreviation rdf:datatype="&xsd;string">FIBO</sm:familyAbbreviation>
        <sm:familyURL rdf:datatype="&xsd;anyURI">http://www.omg.org/spec/EDMC-FIBO/</sm:familyURL>
        <sm:familyAbstract rdf:datatype="&xsd;string">The content that comprises the Financial Industry Business Ontology (FIBO) is documentation, interpretable in formal logic, of the concepts represented by finance industry terms as used in official financial organization documents such as contracts, product/service specifications and governance and regulatory compliance documents.</sm:familyAbstract>

        <sm:technologyArea rdf:datatype="&xsd;string">formal semantics</sm:technologyArea>

        <sm:topicArea rdf:datatype="&xsd;string">finance</sm:topicArea>

        <sm:keyword rdf:datatype="&xsd;string">Financial Industry Business Ontology</sm:keyword>
        <sm:keyword rdf:datatype="&xsd;string">FIBO</sm:keyword>
        <sm:keyword rdf:datatype="&xsd;string">ontology</sm:keyword>
        <sm:keyword rdf:datatype="&xsd;string">vocabulary</sm:keyword>


    <!-- Specification Level Metadata for the FIBO Legal Core Ontology -->

        <sm:specificationTitle rdf:datatype="&xsd;string">Financial Industry Business Ontology (FIBO) Foundations Specification</sm:specificationTitle>
        <sm:specificationAbbreviation rdf:datatype="&xsd;string">FIBO-FND</sm:specificationAbbreviation>
        <sm:specificationURL rdf:datatype="&xsd;anyURI">http://www.omg.org/spec/EDMC-FIBO/FND/</sm:specificationURL>
        <sm:specificationAbstract rdf:datatype="&xsd;string">FIBO Foundations is a set of business concepts which are intended to support the financial industry terms semantics presented in other FIBO specifications.  

The FIBO Foundations models define concepts which are not unique to the financial services industry. From these, financial industry terms in other FIBO specifications may be derived by extension. Terms are also included which may be referred to by properties of things in those specifications. FIBO Foundations therefore includes a number of basic terms about legal, contractual and organizational concepts, among others. </sm:specificationAbstract>

        <sm:dependsOn rdf:datatype="&xsd;anyURI">http://www.omg.org/techprocess/ab/SpecificationMetadata/</sm:dependsOn>

        <sm:keyword rdf:datatype="&xsd;string">foundational vocabulary</sm:keyword>


    <!-- Specification Version Metadata for the FIBO Legal Core Ontology -->

        <sm:thisVersion rdf:datatype="&xsd;string">1.0 </sm:thisVersion>
        <sm:publicationDate rdf:datatype="&xsd;dateTime">2013-08-26T18:00:00</sm:publicationDate>
        <sm:specificationVersionURL rdf:datatype="&xsd;anyURI">http://www.omg.org/spec/EDMC-FIBO/FND/1.0/</sm:specificationVersionURL>
        <sm:specificationVersionStatus rdf:datatype="&xsd;string">Request For Comments (RFC)</sm:specificationVersionStatus>
        <skos:historyNote rdf:datatype="&xsd;string">This version of the FIBO Foundations Specification was revised primarily to reflect comments received at the March 2013 OMG Technical Meeting in Reston and reflected in the Errata discussed at the June 2013 OMG Technical Meeting in Berlin. 

Revisions to FIBO Foundations are managed per the process outlined in the Policies and Procedures for OMG standards, with the intent to maintain backwards compatibility in the ontologies to the degree possible.
  
The RDF/XML serialized OWL for the Foundations ODM/OWL ontologies have been checked for syntactic errors and logical consistency with Protege 4 (http://protege.stanford.edu/), HermiT 1.3.7 (http://www.hermit-reasoner.com/) and Pellet 2.2 (http://clarkparsia.com/pellet/).</skos:historyNote>
        <sm:addressForComments rdf:datatype="&xsd;anyURI">http://www.omg.org/issues/</sm:addressForComments>


    <!-- Module Level Metadata for the FIBO Legal Core Ontology -->

        <sm:moduleName rdf:datatype="&xsd;string">Law</sm:moduleName>
        <sm:moduleAbbreviation rdf:datatype="&xsd;string">FIBO-FND-LAW</sm:moduleAbbreviation>
        <sm:moduleVersion rdf:datatype="&xsd;string">1.0</sm:moduleVersion>
        <sm:moduleAbstract rdf:datatype="&xsd;string">This module includes several ontologies defining legal concepts, including constitutions, laws and jurisdictions. It also includes the definition of legal capacities such as signatory capacity, contractual capability and the like.</sm:moduleAbstract>


    <!-- Curation and Rights Metadata for the FIBO Legal Core Ontology -->

        <sm:copyright rdf:datatype="&xsd;string">Copyright (c) 2013 EDM Council, Inc.
Copyright (c) 2013 Object Management Group, Inc.</sm:copyright>
        <sm:submitter rdf:datatype="&xsd;string">EDM Council, Inc.</sm:submitter>
        <sm:contributor rdf:datatype="&xsd;string">Adaptive, Inc.</sm:contributor>
        <sm:contributor rdf:datatype="&xsd;string">Thematix Partners LLC</sm:contributor>
        <dct:license rdf:datatype="&xsd;string">The MIT License:  Permission is hereby granted, free of charge, to any person obtaining a copy of this software and associated documentation files (the &quot;Software&quot;), to deal in the Software without restriction, including without limitation the rights to use, copy, modify, merge, publish, distribute, sublicense, and/or sell copies of the Software, and to permit persons to whom the Software is furnished to do so, subject to the following conditions:

The copyright notice and this permission notice shall be included in all copies or substantial portions of the Software.

THE SOFTWARE IS PROVIDED &quot;AS IS&quot;, WITHOUT WARRANTY OF ANY KIND, EXPRESS OR IMPLIED, INCLUDING BUT NOT LIMITED TO THE WARRANTIES OF MERCHANTABILITY, FITNESS FOR A PARTICULAR PURPOSE
AND NONINFRINGEMENT.  IN NO EVENT SHALL THE AUTHORS OR COPYRIGHT HOLDERS BE LIABLE FOR ANY CLAIM, DAMAGES OR OTHER LIABILITY, WHETHER IN AN ACTION OF CONTRACT, TORT OR OTHERWISE, ARISING FROM, OUT OF OR IN CONNECTION WITH THE SOFTWARE OR THE USE OR OTHER DEALINGS IN THE SOFTWARE.</dct:license>
        <dct:license rdf:datatype="&xsd;anyURI">http://opensource.org/licenses/mit-license.php</dct:license>
        <sm:responsibleTaskForce rdf:datatype="&xsd;anyURI">http://fdtf.omg.org/</sm:responsibleTaskForce>


    <!-- Ontology/File-Level Metadata for the Legal Core Ontology -->

        <sm:filename rdf:datatype="&xsd;string">Legal Core Ontology</sm:filename>
        <sm:fileAbbreviation rdf:datatype="&xsd;string">fibo-fnd-law-cor</sm:fileAbbreviation>
        <owl:versionIRI rdf:datatype="&xsd;anyURI">http://www.omg.org/spec/EDMC-FIBO/FND/20130801/Law/LegalCore/</owl:versionIRI>
        <sm:priorVersion rdf:datatype="&xsd;anyURI">http://www.omg.org/spec/FIBO/Foundations/20130601/Law/LegalCore.owl</sm:priorVersion>
        <sm:fileAbstract rdf:datatype="&xsd;string">This ontology defines high-level legal concepts for use in other FIBO ontology elements. These concepts include law and constitution, both of which are framed at a more abstract level than national or state laws and constitutions, so that law forms the basis both for statutes and for company by-laws, and constitution forms the basis both for national or state constitutions and for instruments which are constitutive of incorporated legal entities. This ontology also defines some of the variants of these such as governmental constitutions and ordinances. Other types of law are provided in the Jurisdictions ontology as extensions of concepts in this ontology. Court of Law is also defined here.</sm:fileAbstract>
        <skos:changeNote rdf:datatype="&xsd;string">This version of the ontology was revised in advance of the September 2013 New Brunswick, NJ meeting, as follows:
   (1) to use slash style URI/IRIss (also called 303 URIs, vs. hash style) as required to support server side processing 
   (2) to use version-independent IRIs for all definitions internally as opposed to version-specific IRIs
   (3) to change the file suffix from .owl to .rdf to increase usability in RDF tools
   (4) to use 4-level abbreviations and corresponding namespace prefixes for all FIBO ontologies, reflecting a family/specification/module/ontology structure
   (5) to incorporate changes to the specification metadata to support documentation at the family, specification, module, and ontology level, similar to the abbreviations.
   (6) to revise some of the text definitions using more formal sources.</skos:changeNote>

        <sm:dependsOn rdf:datatype="&xsd;anyURI">http://www.omg.org/spec/EDMC-FIBO/FND/Utilities/AnnotationVocabulary/</sm:dependsOn>
        <sm:dependsOn rdf:datatype="&xsd;anyURI">http://www.omg.org/spec/EDMC-FIBO/FND/Utilities/BusinessFacingTypes/</sm:dependsOn>
        <sm:dependsOn rdf:datatype="&xsd;anyURI">http://www.omg.org/spec/EDMC-FIBO/FND/Relations/Relations/</sm:dependsOn>
        <sm:dependsOn rdf:datatype="&xsd;anyURI">http://www.omg.org/spec/EDMC-FIBO/FND/AgentsAndPeople/Agents/</sm:dependsOn>
        <sm:dependsOn rdf:datatype="&xsd;anyURI">http://www.omg.org/spec/EDMC-FIBO/FND/GoalsAndObjectives/Goals/</sm:dependsOn>
        <sm:dependsOn rdf:datatype="&xsd;anyURI">http://www.omg.org/spec/EDMC-FIBO/FND/Places/Locations/</sm:dependsOn>
        <sm:dependsOn rdf:datatype="&xsd;anyURI">http://www.omg.org/spec/EDMC-FIBO/FND/Places/Countries/</sm:dependsOn>
        <sm:dependsOn rdf:datatype="&xsd;anyURI">http://www.omg.org/spec/EDMC-FIBO/FND/Places/Addresses/</sm:dependsOn>
        <sm:dependsOn rdf:datatype="&xsd;anyURI">http://www.omg.org/spec/EDMC-FIBO/FND/Organizations/Organizations/</sm:dependsOn>
        <sm:dependsOn rdf:datatype="&xsd;anyURI">http://www.omg.org/spec/EDMC-FIBO/FND/Organizations/FormalOrganizations/</sm:dependsOn>

        <sm:contentLanguage rdf:datatype="&xsd;anyURI">http://www.w3.org/standards/techs/owl#w3c_all</sm:contentLanguage>
        <sm:contentLanguage rdf:datatype="&xsd;anyURI">http://www.omg.org/spec/ODM/</sm:contentLanguage>


        <owl:imports rdf:resource="http://www.omg.org/techprocess/ab/SpecificationMetadata/"/>
        <owl:imports rdf:resource="http://www.omg.org/spec/EDMC-FIBO/FND/Utilities/AnnotationVocabulary/"/>
        <owl:imports rdf:resource="http://www.omg.org/spec/EDMC-FIBO/FND/Utilities/BusinessFacingTypes/"/>
        <owl:imports rdf:resource="http://www.omg.org/spec/EDMC-FIBO/FND/Relations/Relations/"/>
        <owl:imports rdf:resource="http://www.omg.org/spec/EDMC-FIBO/FND/AgentsAndPeople/Agents/"/>
        <owl:imports rdf:resource="http://www.omg.org/spec/EDMC-FIBO/FND/GoalsAndObjectives/Goals/"/>
        <owl:imports rdf:resource="http://www.omg.org/spec/EDMC-FIBO/FND/Places/Locations/"/>
        <owl:imports rdf:resource="http://www.omg.org/spec/EDMC-FIBO/FND/Places/Countries/"/>
        <owl:imports rdf:resource="http://www.omg.org/spec/EDMC-FIBO/FND/Places/Addresses/"/>
        <owl:imports rdf:resource="http://www.omg.org/spec/EDMC-FIBO/FND/Organizations/Organizations/"/>
        <owl:imports rdf:resource="http://www.omg.org/spec/EDMC-FIBO/FND/Organizations/FormalOrganizations/"/>
    </owl:Ontology>


    <!-- 
    ///////////////////////////////////////////////////////////////////////////////////////
    //
    // Classes
    //
    ///////////////////////////////////////////////////////////////////////////////////////
     -->

    <owl:Class rdf:about="&fibo-fnd-law-cor;Constitution">
        <rdfs:label>constitution</rdfs:label>
        <skos:definition>A constitution defines the basic principles and laws of a nation, state, or social group that determine the powers and duties of the government and guarantee certain rights to the people in it.</skos:definition>
        <skos:editorialNote>This defines the framework in which laws (for a country constitution), rules and regulations (for a party or organization constitution) or contractual commitments are made and in which they have force.</skos:editorialNote>
        <fibo-fnd-utl-av:definitionOrigin>Merriam-Webster Online Dictionary</fibo-fnd-utl-av:definitionOrigin>
        <rdfs:subClassOf>
             <owl:Restriction>
                 <owl:onProperty rdf:resource="&fibo-fnd-rel-rel;governs"/>
                 <owl:allValuesFrom rdf:resource="&fibo-fnd-law-cor;Law"/>
             </owl:Restriction>
        </rdfs:subClassOf>
    </owl:Class>

    <owl:Class rdf:about="&fibo-fnd-law-cor;CourtOfLaw">
        <rdfs:label>court of law</rdfs:label>
        <skos:definition>A court of law is a court that hears cases and decides them on the basis of statutes or the common law.</skos:definition>
        <fibo-fnd-utl-av:definitionOrigin>Merriam-Webster Online Dictionary</fibo-fnd-utl-av:definitionOrigin>
        <rdfs:subClassOf rdf:resource="&fibo-fnd-org-fm;FormalOrganization"/>
    </owl:Class>

    <owl:Class rdf:about="&fibo-fnd-law-cor;Law">
        <rdfs:label>Law</rdfs:label>
        <skos:definition>Law is a term which does not have a universally accepted definition, but one definition is that law is a system of rules and guidelines which are enforced through social institutions to govern behavior. Laws are made by governments, specifically by their legislatures.  The formation of laws themselves may be influenced by a constitution (written or unwritten) and the rights encoded therein.  The law shapes politics, economics and society in countless ways and serves as a social mediator of relations between people.</skos:definition>
        <fibo-fnd-utl-av:definitionOrigin>http://en.wikipedia.org/wiki/Law</fibo-fnd-utl-av:definitionOrigin>
        <skos:editorialNote>Any law or body of law, which may have force in some context, including national laws, company bylaws and the like.</skos:editorialNote>
    </owl:Class>

    <owl:Class rdf:about="&fibo-fnd-law-cor;GovernmentalConstitution">
        <rdfs:label>governmental constitution</rdfs:label>
        <skos:definition>Most commonly, the term constitution refers to a set of rules and principles that define the nature and extent of government.  Most constitutions seek to regulate the relationship between institutions of the state, in a basic sense the relationship between the executive, legislature and the judiciary, but also the relationship of institutions within those branches.  For example, executive branches can be divided into a head of government, government departments/ministries, executive agencies and a civil service/administration.  Most constitutions also attempt to define the relationship between individuals and the state, and to establish the broad rights of individual citizens. It is thus the most basic law of a territory from which all the other laws and rules are hierarchically derived; in some territories it is in fact called Basic Law.</skos:definition>
        <fibo-fnd-utl-av:definitionOrigin>http://en.wikipedia.org/wiki/Constitution#Governmental_constitutions</fibo-fnd-utl-av:definitionOrigin>
        <skos:editorialNote>This defines the framework in which laws are made and in which they have force.</skos:editorialNote>
        <rdfs:subClassOf rdf:resource="&fibo-fnd-law-cor;Constitution"/>
    </owl:Class>

    <owl:Class rdf:about="&fibo-fnd-law-cor;Ordinance">
        <rdfs:label>ordinance</rdfs:label>
        <skos:definition>An authoritative rule or law; a decree or command; a public injunction or regulation, such as a city ordinance against excessive horn blowing. (Source: Dictionary.com)</skos:definition>
        <rdfs:subClassOf rdf:resource="&fibo-fnd-law-cor;Law"/>
    </owl:Class>

</rdf:RDF>