<?xml version="1.0" encoding="UTF-8"?>
<rdf:RDF xmlns:xsd="http://www.w3.org/2001/XMLSchema#"
         xmlns:sm="http://www.omg.org/techprocess/ab/SpecificationMetadata/"
         xmlns:fibo-fnd-utl-av="http://www.omg.org/spec/EDMC-FIBO/FND/Utilities/AnnotationVocabulary/"
         xmlns:rdf="http://www.w3.org/1999/02/22-rdf-syntax-ns#"
         xmlns:rdfs="http://www.w3.org/2000/01/rdf-schema#"
         xmlns:owl="http://www.w3.org/2002/07/owl#"
         xmlns:skos="http://www.w3.org/2004/02/skos/core#"
         xmlns:dc="http://purl.org/dc/terms/"
         xml:base="http://www.edmcouncil.org/spec/EDMC-SR/FND/Relative/QuantifiedResources/">

   <owl:Ontology rdf:about="http://www.edmcouncil.org/spec/EDMC-SR/FND/Relative/QuantifiedResources/">
      <owl:imports rdf:resource="http://www.edmcouncil.org/spec/EDMC-SR/FND/Math/Amounts/"/>
      <owl:imports rdf:resource="http://www.edmcouncil.org/spec/EDMC-SR/FND/Relative/EconomicResources/"/>
      <owl:imports rdf:resource="http://www.edmcouncil.org/spec/EDMC-SR/FND/Relative/ToolsAndInstruments/"/>
   </owl:Ontology>

   <!--Datatypes-->

<!--Object Properties-->

<owl:ObjectProperty rdf:about="http://www.edmcouncil.org/spec/EDMC-SR/FND/Relative/QuantifiedResources/quantifiedRawMaterialTakesMaterialForm">
      <skos:definition>The actual numerical amount of some material, that is represented as quantified raw material.</skos:definition>
      <rdfs:subPropertyOf rdf:resource="http://www.edmcouncil.org/spec/EDMC-SR/FND/Relative/QuantifiedResources/quantifiedResourceTakesMaterialForm"/>
      <rdfs:domain rdf:resource="http://www.edmcouncil.org/spec/EDMC-SR/FND/Relative/QuantifiedResources/QuantifiedRawMaterial"/>
      <rdfs:range rdf:resource="http://www.edmcouncil.org/spec/EDMC-SR/FND/Math/Amounts/MaterialAmount"/>
   </owl:ObjectProperty>

   <owl:ObjectProperty rdf:about="http://www.edmcouncil.org/spec/EDMC-SR/FND/Relative/QuantifiedResources/quantifiedResourceTakesMaterialForm">
      <skos:definition>The actual numerical amount of something, that is represented by the quantified resource, e.g. the amount of money that is represented by an amount of Capital, or the amount of goods or raw material. .</skos:definition>
      <rdfs:subPropertyOf rdf:resource="http://www.edmcouncil.org/spec/EDMC-SR/FND/Relative/EconomicResources/takesMaterialForm"/>
      <rdfs:domain rdf:resource="http://www.edmcouncil.org/spec/EDMC-SR/FND/Relative/QuantifiedResources/QuantifiedResource"/>
      <rdfs:range rdf:resource="http://www.edmcouncil.org/spec/EDMC-SR/FND/Math/Amounts/NumericAmount"/>
   </owl:ObjectProperty>

   <!--Data Properties-->

<!--Annotation Properties-->

<!--Classes-->

<owl:Class rdf:about="http://www.edmcouncil.org/spec/EDMC-SR/FND/Relative/QuantifiedResources/QuantifiedRawMaterial">
      <rdfs:label>Quantified Raw Material</rdfs:label>
      <skos:definition>Some measured or quantified amount of some raw material. Scope Note: This is a kind of economic resource i.e. it may be bought or sold or exchanged, or put to work in some process.</skos:definition>
      <rdfs:subClassOf rdf:resource="http://www.edmcouncil.org/spec/EDMC-SR/FND/Relative/QuantifiedResources/QuantifiedResource"/>
   </owl:Class>

   <owl:Class rdf:about="http://www.edmcouncil.org/spec/EDMC-SR/FND/Relative/QuantifiedResources/QuantifiedResource">
      <rdfs:label>Quantified Resource</rdfs:label>
      <skos:definition>An amount of something which is defined in terms of its use for some purpose.</skos:definition>
      <skos:editorialNote>An example would be Capital, which is an amount of money with a purpose.</skos:editorialNote>
      <rdfs:subClassOf rdf:resource="http://www.edmcouncil.org/spec/EDMC-SR/FND/Relative/EconomicResources/EconomicResource"/>
   </owl:Class>

   <!--Individuals-->

</rdf:RDF>