<?xml version="1.0" encoding="UTF-8"?>
<!DOCTYPE rdf:RDF [
	<!ENTITY cmns-av "https://www.omg.org/spec/Commons/AnnotationVocabulary/">
	<!ENTITY cmns-cls "https://www.omg.org/spec/Commons/Classifiers/">
	<!ENTITY cmns-col "https://www.omg.org/spec/Commons/Collections/">
	<!ENTITY cmns-cxtdsg "https://www.omg.org/spec/Commons/ContextualDesignators/">
	<!ENTITY cmns-doc "https://www.omg.org/spec/Commons/Documents/">
	<!ENTITY cmns-dsg "https://www.omg.org/spec/Commons/Designators/">
	<!ENTITY cmns-dt "https://www.omg.org/spec/Commons/DatesAndTimes/">
	<!ENTITY cmns-loc "https://www.omg.org/spec/Commons/Locations/">
	<!ENTITY cmns-org "https://www.omg.org/spec/Commons/Organizations/">
	<!ENTITY cmns-pts "https://www.omg.org/spec/Commons/PartiesAndSituations/">
	<!ENTITY cmns-qtu "https://www.omg.org/spec/Commons/QuantitiesAndUnits/">
	<!ENTITY cmns-rga "https://www.omg.org/spec/Commons/RegulatoryAgencies/">
	<!ENTITY cmns-rlcmp "https://www.omg.org/spec/Commons/RolesAndCompositions/">
	<!ENTITY dct "http://purl.org/dc/terms/">
	<!ENTITY fibo-be-fct-pub "https://spec.edmcouncil.org/fibo/ontology/BE/FunctionalEntities/Publishers/">
	<!ENTITY fibo-be-ge-euj "https://spec.edmcouncil.org/fibo/ontology/BE/GovernmentEntities/EuropeanJurisdiction/EUGovernmentEntitiesAndJurisdictions/">
	<!ENTITY fibo-be-le-cb "https://spec.edmcouncil.org/fibo/ontology/BE/LegalEntities/CorporateBodies/">
	<!ENTITY fibo-be-le-fbo "https://spec.edmcouncil.org/fibo/ontology/BE/LegalEntities/FormalBusinessOrganizations/">
	<!ENTITY fibo-be-le-lp "https://spec.edmcouncil.org/fibo/ontology/BE/LegalEntities/LegalPersons/">
	<!ENTITY fibo-be-oac-cown "https://spec.edmcouncil.org/fibo/ontology/BE/OwnershipAndControl/CorporateOwnership/">
	<!ENTITY fibo-be-oac-opty "https://spec.edmcouncil.org/fibo/ontology/BE/OwnershipAndControl/OwnershipParties/">
	<!ENTITY fibo-fbc-dae-dbt "https://spec.edmcouncil.org/fibo/ontology/FBC/DebtAndEquities/Debt/">
	<!ENTITY fibo-fbc-fi-fi "https://spec.edmcouncil.org/fibo/ontology/FBC/FinancialInstruments/FinancialInstruments/">
	<!ENTITY fibo-fbc-fi-stl "https://spec.edmcouncil.org/fibo/ontology/FBC/FinancialInstruments/Settlement/">
	<!ENTITY fibo-fbc-pas-caa "https://spec.edmcouncil.org/fibo/ontology/FBC/ProductsAndServices/ClientsAndAccounts/">
	<!ENTITY fibo-fbc-pas-fpas "https://spec.edmcouncil.org/fibo/ontology/FBC/ProductsAndServices/FinancialProductsAndServices/">
	<!ENTITY fibo-fnd-acc-aeq "https://spec.edmcouncil.org/fibo/ontology/FND/Accounting/AccountingEquity/">
	<!ENTITY fibo-fnd-acc-cur "https://spec.edmcouncil.org/fibo/ontology/FND/Accounting/CurrencyAmount/">
	<!ENTITY fibo-fnd-agr-ctr "https://spec.edmcouncil.org/fibo/ontology/FND/Agreements/Contracts/">
	<!ENTITY fibo-fnd-arr-lif "https://spec.edmcouncil.org/fibo/ontology/FND/Arrangements/Lifecycles/">
	<!ENTITY fibo-fnd-arr-rt "https://spec.edmcouncil.org/fibo/ontology/FND/Arrangements/Ratings/">
	<!ENTITY fibo-fnd-dt-bd "https://spec.edmcouncil.org/fibo/ontology/FND/DatesAndTimes/BusinessDates/">
	<!ENTITY fibo-fnd-dt-fd "https://spec.edmcouncil.org/fibo/ontology/FND/DatesAndTimes/FinancialDates/">
	<!ENTITY fibo-fnd-gao-obj "https://spec.edmcouncil.org/fibo/ontology/FND/GoalsAndObjectives/Objectives/">
	<!ENTITY fibo-fnd-law-cor "https://spec.edmcouncil.org/fibo/ontology/FND/Law/LegalCore/">
	<!ENTITY fibo-fnd-law-lcap "https://spec.edmcouncil.org/fibo/ontology/FND/Law/LegalCapacity/">
	<!ENTITY fibo-fnd-oac-own "https://spec.edmcouncil.org/fibo/ontology/FND/OwnershipAndControl/Ownership/">
	<!ENTITY fibo-fnd-plc-rp "https://spec.edmcouncil.org/fibo/ontology/FND/Places/RealProperty/">
	<!ENTITY fibo-fnd-rel-rel "https://spec.edmcouncil.org/fibo/ontology/FND/Relations/Relations/">
	<!ENTITY fibo-fnd-utl-av "https://spec.edmcouncil.org/fibo/ontology/FND/Utilities/AnnotationVocabulary/">
	<!ENTITY fibo-ind-ind-ind "https://spec.edmcouncil.org/fibo/ontology/IND/Indicators/Indicators/">
	<!ENTITY fibo-sec-eq-eq "https://spec.edmcouncil.org/fibo/ontology/SEC/Equities/EquityInstruments/">
	<!ENTITY fibo-sec-fund-civ "https://spec.edmcouncil.org/fibo/ontology/SEC/Funds/CollectiveInvestmentVehicles/">
	<!ENTITY fibo-sec-fund-fund "https://spec.edmcouncil.org/fibo/ontology/SEC/Funds/Funds/">
	<!ENTITY fibo-sec-sec-ast "https://spec.edmcouncil.org/fibo/ontology/SEC/Securities/SecurityAssets/">
	<!ENTITY fibo-sec-sec-cls "https://spec.edmcouncil.org/fibo/ontology/SEC/Securities/SecuritiesClassification/">
	<!ENTITY fibo-sec-sec-iss "https://spec.edmcouncil.org/fibo/ontology/SEC/Securities/SecuritiesIssuance/">
	<!ENTITY fibo-sec-sec-pls "https://spec.edmcouncil.org/fibo/ontology/SEC/Securities/Pools/">
	<!ENTITY fibo-sec-sec-rst "https://spec.edmcouncil.org/fibo/ontology/SEC/Securities/SecuritiesRestrictions/">
	<!ENTITY owl "http://www.w3.org/2002/07/owl#">
	<!ENTITY rdf "http://www.w3.org/1999/02/22-rdf-syntax-ns#">
	<!ENTITY rdfs "http://www.w3.org/2000/01/rdf-schema#">
	<!ENTITY skos "http://www.w3.org/2004/02/skos/core#">
	<!ENTITY xsd "http://www.w3.org/2001/XMLSchema#">
]>
<rdf:RDF xml:base="https://spec.edmcouncil.org/fibo/ontology/SEC/Funds/CollectiveInvestmentVehicles/"
	xmlns:cmns-av="https://www.omg.org/spec/Commons/AnnotationVocabulary/"
	xmlns:cmns-cls="https://www.omg.org/spec/Commons/Classifiers/"
	xmlns:cmns-col="https://www.omg.org/spec/Commons/Collections/"
	xmlns:cmns-cxtdsg="https://www.omg.org/spec/Commons/ContextualDesignators/"
	xmlns:cmns-doc="https://www.omg.org/spec/Commons/Documents/"
	xmlns:cmns-dsg="https://www.omg.org/spec/Commons/Designators/"
	xmlns:cmns-dt="https://www.omg.org/spec/Commons/DatesAndTimes/"
	xmlns:cmns-loc="https://www.omg.org/spec/Commons/Locations/"
	xmlns:cmns-org="https://www.omg.org/spec/Commons/Organizations/"
	xmlns:cmns-pts="https://www.omg.org/spec/Commons/PartiesAndSituations/"
	xmlns:cmns-qtu="https://www.omg.org/spec/Commons/QuantitiesAndUnits/"
	xmlns:cmns-rga="https://www.omg.org/spec/Commons/RegulatoryAgencies/"
	xmlns:cmns-rlcmp="https://www.omg.org/spec/Commons/RolesAndCompositions/"
	xmlns:dct="http://purl.org/dc/terms/"
	xmlns:fibo-be-fct-pub="https://spec.edmcouncil.org/fibo/ontology/BE/FunctionalEntities/Publishers/"
	xmlns:fibo-be-ge-euj="https://spec.edmcouncil.org/fibo/ontology/BE/GovernmentEntities/EuropeanJurisdiction/EUGovernmentEntitiesAndJurisdictions/"
	xmlns:fibo-be-le-cb="https://spec.edmcouncil.org/fibo/ontology/BE/LegalEntities/CorporateBodies/"
	xmlns:fibo-be-le-fbo="https://spec.edmcouncil.org/fibo/ontology/BE/LegalEntities/FormalBusinessOrganizations/"
	xmlns:fibo-be-le-lp="https://spec.edmcouncil.org/fibo/ontology/BE/LegalEntities/LegalPersons/"
	xmlns:fibo-be-oac-cown="https://spec.edmcouncil.org/fibo/ontology/BE/OwnershipAndControl/CorporateOwnership/"
	xmlns:fibo-be-oac-opty="https://spec.edmcouncil.org/fibo/ontology/BE/OwnershipAndControl/OwnershipParties/"
	xmlns:fibo-fbc-dae-dbt="https://spec.edmcouncil.org/fibo/ontology/FBC/DebtAndEquities/Debt/"
	xmlns:fibo-fbc-fi-fi="https://spec.edmcouncil.org/fibo/ontology/FBC/FinancialInstruments/FinancialInstruments/"
	xmlns:fibo-fbc-fi-stl="https://spec.edmcouncil.org/fibo/ontology/FBC/FinancialInstruments/Settlement/"
	xmlns:fibo-fbc-pas-caa="https://spec.edmcouncil.org/fibo/ontology/FBC/ProductsAndServices/ClientsAndAccounts/"
	xmlns:fibo-fbc-pas-fpas="https://spec.edmcouncil.org/fibo/ontology/FBC/ProductsAndServices/FinancialProductsAndServices/"
	xmlns:fibo-fnd-acc-aeq="https://spec.edmcouncil.org/fibo/ontology/FND/Accounting/AccountingEquity/"
	xmlns:fibo-fnd-acc-cur="https://spec.edmcouncil.org/fibo/ontology/FND/Accounting/CurrencyAmount/"
	xmlns:fibo-fnd-agr-ctr="https://spec.edmcouncil.org/fibo/ontology/FND/Agreements/Contracts/"
	xmlns:fibo-fnd-arr-lif="https://spec.edmcouncil.org/fibo/ontology/FND/Arrangements/Lifecycles/"
	xmlns:fibo-fnd-arr-rt="https://spec.edmcouncil.org/fibo/ontology/FND/Arrangements/Ratings/"
	xmlns:fibo-fnd-dt-bd="https://spec.edmcouncil.org/fibo/ontology/FND/DatesAndTimes/BusinessDates/"
	xmlns:fibo-fnd-dt-fd="https://spec.edmcouncil.org/fibo/ontology/FND/DatesAndTimes/FinancialDates/"
	xmlns:fibo-fnd-gao-obj="https://spec.edmcouncil.org/fibo/ontology/FND/GoalsAndObjectives/Objectives/"
	xmlns:fibo-fnd-law-cor="https://spec.edmcouncil.org/fibo/ontology/FND/Law/LegalCore/"
	xmlns:fibo-fnd-law-lcap="https://spec.edmcouncil.org/fibo/ontology/FND/Law/LegalCapacity/"
	xmlns:fibo-fnd-oac-own="https://spec.edmcouncil.org/fibo/ontology/FND/OwnershipAndControl/Ownership/"
	xmlns:fibo-fnd-plc-rp="https://spec.edmcouncil.org/fibo/ontology/FND/Places/RealProperty/"
	xmlns:fibo-fnd-rel-rel="https://spec.edmcouncil.org/fibo/ontology/FND/Relations/Relations/"
	xmlns:fibo-fnd-utl-av="https://spec.edmcouncil.org/fibo/ontology/FND/Utilities/AnnotationVocabulary/"
	xmlns:fibo-ind-ind-ind="https://spec.edmcouncil.org/fibo/ontology/IND/Indicators/Indicators/"
	xmlns:fibo-sec-eq-eq="https://spec.edmcouncil.org/fibo/ontology/SEC/Equities/EquityInstruments/"
	xmlns:fibo-sec-fund-civ="https://spec.edmcouncil.org/fibo/ontology/SEC/Funds/CollectiveInvestmentVehicles/"
	xmlns:fibo-sec-fund-fund="https://spec.edmcouncil.org/fibo/ontology/SEC/Funds/Funds/"
	xmlns:fibo-sec-sec-ast="https://spec.edmcouncil.org/fibo/ontology/SEC/Securities/SecurityAssets/"
	xmlns:fibo-sec-sec-cls="https://spec.edmcouncil.org/fibo/ontology/SEC/Securities/SecuritiesClassification/"
	xmlns:fibo-sec-sec-iss="https://spec.edmcouncil.org/fibo/ontology/SEC/Securities/SecuritiesIssuance/"
	xmlns:fibo-sec-sec-pls="https://spec.edmcouncil.org/fibo/ontology/SEC/Securities/Pools/"
	xmlns:fibo-sec-sec-rst="https://spec.edmcouncil.org/fibo/ontology/SEC/Securities/SecuritiesRestrictions/"
	xmlns:owl="http://www.w3.org/2002/07/owl#"
	xmlns:rdf="http://www.w3.org/1999/02/22-rdf-syntax-ns#"
	xmlns:rdfs="http://www.w3.org/2000/01/rdf-schema#"
	xmlns:skos="http://www.w3.org/2004/02/skos/core#"
	xmlns:xsd="http://www.w3.org/2001/XMLSchema#">
	
	<owl:Ontology rdf:about="https://spec.edmcouncil.org/fibo/ontology/SEC/Funds/CollectiveInvestmentVehicles/">
		<rdfs:label xml:lang="en">Collective Investment Vehicles Ontology</rdfs:label>
		<dct:abstract>Reference data terms and non time dependent facts about funds and CIVs.</dct:abstract>
		<dct:license>Copyright (c) 2013-2025 EDM Council, Inc.
Copyright (c) 2013-2025 Object Management Group, Inc.

Permission is hereby granted, free of charge, to any person obtaining a copy of this software and associated documentation files (the &apos;Software&apos;), to deal in the Software without restriction, including without limitation the rights to use, copy, modify, merge, publish, distribute, sublicense, and/or sell copies of the Software, and to permit persons to whom the Software is furnished to do so, subject to the following conditions:

The above copyright notice and this permission notice shall be included in all copies or substantial portions of the Software.

THE SOFTWARE IS PROVIDED &apos;AS IS&apos;, WITHOUT WARRANTY OF ANY KIND, EXPRESS OR IMPLIED, INCLUDING BUT NOT LIMITED TO THE WARRANTIES OF MERCHANTABILITY, FITNESS FOR A PARTICULAR PURPOSE AND NONINFRINGEMENT. IN NO EVENT SHALL THE AUTHORS OR COPYRIGHT HOLDERS BE LIABLE FOR ANY CLAIM, DAMAGES OR OTHER LIABILITY, WHETHER IN AN ACTION OF CONTRACT, TORT OR OTHERWISE, ARISING FROM, OUT OF OR IN CONNECTION WITH THE SOFTWARE OR THE USE OR OTHER DEALINGS IN THE SOFTWARE.
		
		See https://opensource.org/licenses/MIT.</dct:license>
		<owl:imports rdf:resource="https://spec.edmcouncil.org/fibo/ontology/BE/FunctionalEntities/Publishers/"/>
		<owl:imports rdf:resource="https://spec.edmcouncil.org/fibo/ontology/BE/GovernmentEntities/EuropeanJurisdiction/EUGovernmentEntitiesAndJurisdictions/"/>
		<owl:imports rdf:resource="https://spec.edmcouncil.org/fibo/ontology/BE/LegalEntities/CorporateBodies/"/>
		<owl:imports rdf:resource="https://spec.edmcouncil.org/fibo/ontology/BE/LegalEntities/FormalBusinessOrganizations/"/>
		<owl:imports rdf:resource="https://spec.edmcouncil.org/fibo/ontology/BE/LegalEntities/LegalPersons/"/>
		<owl:imports rdf:resource="https://spec.edmcouncil.org/fibo/ontology/BE/OwnershipAndControl/CorporateOwnership/"/>
		<owl:imports rdf:resource="https://spec.edmcouncil.org/fibo/ontology/BE/OwnershipAndControl/OwnershipParties/"/>
		<owl:imports rdf:resource="https://spec.edmcouncil.org/fibo/ontology/FBC/DebtAndEquities/Debt/"/>
		<owl:imports rdf:resource="https://spec.edmcouncil.org/fibo/ontology/FBC/FinancialInstruments/FinancialInstruments/"/>
		<owl:imports rdf:resource="https://spec.edmcouncil.org/fibo/ontology/FBC/FinancialInstruments/Settlement/"/>
		<owl:imports rdf:resource="https://spec.edmcouncil.org/fibo/ontology/FBC/ProductsAndServices/ClientsAndAccounts/"/>
		<owl:imports rdf:resource="https://spec.edmcouncil.org/fibo/ontology/FBC/ProductsAndServices/FinancialProductsAndServices/"/>
		<owl:imports rdf:resource="https://spec.edmcouncil.org/fibo/ontology/FND/Accounting/AccountingEquity/"/>
		<owl:imports rdf:resource="https://spec.edmcouncil.org/fibo/ontology/FND/Accounting/CurrencyAmount/"/>
		<owl:imports rdf:resource="https://spec.edmcouncil.org/fibo/ontology/FND/Agreements/Contracts/"/>
		<owl:imports rdf:resource="https://spec.edmcouncil.org/fibo/ontology/FND/Arrangements/Lifecycles/"/>
		<owl:imports rdf:resource="https://spec.edmcouncil.org/fibo/ontology/FND/Arrangements/Ratings/"/>
		<owl:imports rdf:resource="https://spec.edmcouncil.org/fibo/ontology/FND/DatesAndTimes/BusinessDates/"/>
		<owl:imports rdf:resource="https://spec.edmcouncil.org/fibo/ontology/FND/DatesAndTimes/FinancialDates/"/>
		<owl:imports rdf:resource="https://spec.edmcouncil.org/fibo/ontology/FND/GoalsAndObjectives/Objectives/"/>
		<owl:imports rdf:resource="https://spec.edmcouncil.org/fibo/ontology/FND/Law/LegalCapacity/"/>
		<owl:imports rdf:resource="https://spec.edmcouncil.org/fibo/ontology/FND/Law/LegalCore/"/>
		<owl:imports rdf:resource="https://spec.edmcouncil.org/fibo/ontology/FND/OwnershipAndControl/Ownership/"/>
		<owl:imports rdf:resource="https://spec.edmcouncil.org/fibo/ontology/FND/Places/RealProperty/"/>
		<owl:imports rdf:resource="https://spec.edmcouncil.org/fibo/ontology/FND/Relations/Relations/"/>
		<owl:imports rdf:resource="https://spec.edmcouncil.org/fibo/ontology/FND/Utilities/AnnotationVocabulary/"/>
		<owl:imports rdf:resource="https://spec.edmcouncil.org/fibo/ontology/IND/Indicators/Indicators/"/>
		<owl:imports rdf:resource="https://spec.edmcouncil.org/fibo/ontology/SEC/Equities/EquityInstruments/"/>
		<owl:imports rdf:resource="https://spec.edmcouncil.org/fibo/ontology/SEC/Funds/Funds/"/>
		<owl:imports rdf:resource="https://spec.edmcouncil.org/fibo/ontology/SEC/Securities/Pools/"/>
		<owl:imports rdf:resource="https://spec.edmcouncil.org/fibo/ontology/SEC/Securities/SecuritiesClassification/"/>
		<owl:imports rdf:resource="https://spec.edmcouncil.org/fibo/ontology/SEC/Securities/SecuritiesIdentification/"/>
		<owl:imports rdf:resource="https://spec.edmcouncil.org/fibo/ontology/SEC/Securities/SecuritiesIssuance/"/>
		<owl:imports rdf:resource="https://spec.edmcouncil.org/fibo/ontology/SEC/Securities/SecuritiesRestrictions/"/>
		<owl:imports rdf:resource="https://spec.edmcouncil.org/fibo/ontology/SEC/Securities/SecurityAssets/"/>
		<owl:imports rdf:resource="https://www.omg.org/spec/Commons/AnnotationVocabulary/"/>
		<owl:imports rdf:resource="https://www.omg.org/spec/Commons/Classifiers/"/>
		<owl:imports rdf:resource="https://www.omg.org/spec/Commons/Collections/"/>
		<owl:imports rdf:resource="https://www.omg.org/spec/Commons/ContextualDesignators/"/>
		<owl:imports rdf:resource="https://www.omg.org/spec/Commons/DatesAndTimes/"/>
		<owl:imports rdf:resource="https://www.omg.org/spec/Commons/Designators/"/>
		<owl:imports rdf:resource="https://www.omg.org/spec/Commons/Documents/"/>
		<owl:imports rdf:resource="https://www.omg.org/spec/Commons/Locations/"/>
		<owl:imports rdf:resource="https://www.omg.org/spec/Commons/Organizations/"/>
		<owl:imports rdf:resource="https://www.omg.org/spec/Commons/PartiesAndSituations/"/>
		<owl:imports rdf:resource="https://www.omg.org/spec/Commons/QuantitiesAndUnits/"/>
		<owl:imports rdf:resource="https://www.omg.org/spec/Commons/RegulatoryAgencies/"/>
		<owl:imports rdf:resource="https://www.omg.org/spec/Commons/RolesAndCompositions/"/>
		<owl:imports rdf:resource="https://www.omg.org/spec/LCC/Countries/CountryRepresentation/"/>
		<owl:versionIRI rdf:resource="https://spec.edmcouncil.org/fibo/ontology/SEC/Funds/CollectiveInvestmentVehicles/"/>
		<fibo-fnd-utl-av:hasMaturityLevel rdf:resource="&fibo-fnd-utl-av;Provisional"/>
		<cmns-av:copyright>Copyright (c) 2013-2025 EDM Council, Inc.</cmns-av:copyright>
		<cmns-av:copyright>Copyright (c) 2013-2025 Object Management Group, Inc.</cmns-av:copyright>
	</owl:Ontology>
	
	<owl:Class rdf:about="&fibo-sec-fund-civ;AccumulatingShareClass">
		<rdfs:subClassOf rdf:resource="&fibo-sec-fund-civ;FundShareClassUnit"/>
		<rdfs:label xml:lang="en">accumulating share class</rdfs:label>
		<owl:disjointWith rdf:resource="&fibo-sec-fund-civ;DistributingShareClass"/>
		<skos:definition xml:lang="en">A share class in which there is no option to reinvest.</skos:definition>
		<cmns-av:explanatoryNote xml:lang="en">This fact would be determined by the fund unit having a specific Fund Distribution Policy of Accumulating.</cmns-av:explanatoryNote>
	</owl:Class>
	
	<owl:Class rdf:about="&fibo-sec-fund-civ;AssetClassStrategy">
		<rdfs:subClassOf rdf:resource="&fibo-sec-fund-civ;FundPortfolioInvestmentLimitations"/>
		<rdfs:subClassOf>
			<owl:Restriction>
				<owl:onProperty rdf:resource="&fibo-sec-fund-civ;identifiesAssetTypesBy"/>
				<owl:someValuesFrom rdf:resource="&fibo-sec-sec-cls;FinancialInstrumentClassifier"/>
			</owl:Restriction>
		</rdfs:subClassOf>
		<rdfs:label xml:lang="en">asset class strategy</rdfs:label>
		<skos:definition xml:lang="en">Strategy which is asset class based.</skos:definition>
		<cmns-av:explanatoryNote xml:lang="en">EFAMA: The type of securities or other holdings that may be invested in. FIBIM: Strategy which is asset class based. Can implement this in terms of a classification of those things. Wording implies this is a policy.</cmns-av:explanatoryNote>
	</owl:Class>
	
	<owl:Class rdf:about="&fibo-sec-fund-civ;CommonShareInFund">
		<rdfs:subClassOf rdf:resource="&fibo-sec-fund-civ;FundShareClassUnit"/>
		<rdfs:label xml:lang="en">common share in fund</rdfs:label>
		<owl:disjointWith rdf:resource="&fibo-sec-fund-civ;PreferredShareInFund"/>
		<skos:definition xml:lang="en">A share unit in a fund, which is classified as a Common Share class.</skos:definition>
		<cmns-av:explanatoryNote xml:lang="en">SR Review session notes: US: Closed and open ended funds may have common and preferred shares.</cmns-av:explanatoryNote>
	</owl:Class>
	
	<owl:Class rdf:about="&fibo-sec-fund-civ;CurrencyStrategy">
		<rdfs:subClassOf rdf:resource="&fibo-sec-fund-civ;FundPortfolioInvestmentLimitations"/>
		<rdfs:label xml:lang="en">currency strategy</rdfs:label>
		<skos:definition xml:lang="en">Strategy which is currency based.</skos:definition>
	</owl:Class>
	
	<owl:Class rdf:about="&fibo-sec-fund-civ;DebtStakeInFund">
		<rdfs:subClassOf rdf:resource="&fibo-sec-fund-civ;StakeInFund"/>
		<rdfs:label xml:lang="en">debt stake in fund</rdfs:label>
		<skos:definition xml:lang="en">A stake held in a fund by way of a Bond Unit.</skos:definition>
		<cmns-av:explanatoryNote xml:lang="en">Note that you cannot buy fractional amounts in a bond. Review Session Note: Similar to what happens in a CDO where the collaterial manager and the issuer are two different entities. So model this along the same lines as the SPV in the structured finance model. Therefore: further modeling and review required</cmns-av:explanatoryNote>
	</owl:Class>
	
	<owl:Class rdf:about="&fibo-sec-fund-civ;DistributingShareClass">
		<rdfs:subClassOf rdf:resource="&fibo-sec-fund-civ;FundShareClassUnit"/>
		<rdfs:label xml:lang="en">distributing share class</rdfs:label>
	</owl:Class>
	
	<owl:Class rdf:about="&fibo-sec-fund-civ;EquityFund">
		<rdfs:subClassOf rdf:resource="&fibo-sec-sec-pls;CollectiveInvestmentVehicle"/>
		<rdfs:subClassOf>
			<owl:Restriction>
				<owl:onProperty rdf:resource="&cmns-col;comprises"/>
				<owl:someValuesFrom rdf:resource="&fibo-sec-fund-civ;EquityPortfolio"/>
			</owl:Restriction>
		</rdfs:subClassOf>
		<rdfs:label xml:lang="en">equity fund</rdfs:label>
		<skos:definition xml:lang="en">A fund which invests in at least 85% shares.</skos:definition>
	</owl:Class>
	
	<owl:Class rdf:about="&fibo-sec-fund-civ;EquityPortfolio">
		<rdfs:subClassOf rdf:resource="&fibo-sec-fund-civ;FundPortfolio"/>
		<rdfs:subClassOf>
			<owl:Restriction>
				<owl:onProperty rdf:resource="&cmns-col;comprises"/>
				<owl:someValuesFrom rdf:resource="&fibo-be-oac-cown;Shareholding"/>
			</owl:Restriction>
		</rdfs:subClassOf>
		<rdfs:label xml:lang="en">equity portfolio</rdfs:label>
		<skos:definition xml:lang="en">A portfolio which has at least 85% exposure to shares.</skos:definition>
	</owl:Class>
	
	<owl:Class rdf:about="&fibo-sec-fund-civ;EquityStakeInFund">
		<rdfs:subClassOf rdf:resource="&fibo-sec-fund-civ;StakeInFund"/>
		<rdfs:label xml:lang="en">equity stake in fund</rdfs:label>
		<skos:definition xml:lang="en">A stake held in a fund by way of a Share Class Unit.</skos:definition>
		<cmns-av:explanatoryNote xml:lang="en">Theoretically you can buy a fraction of a share in a fund. This would depend on the legal structure of the fund, e.g. a minimum investment. There is always a distribution plan.</cmns-av:explanatoryNote>
	</owl:Class>
	
	<owl:Class rdf:about="&fibo-sec-fund-civ;FondsCommunDePlacement">
		<rdfs:subClassOf rdf:resource="&fibo-sec-sec-pls;CollectiveInvestmentVehicle"/>
		<rdfs:label xml:lang="fr-FR">fonds commun de placement</rdfs:label>
		<rdfs:seeAlso rdf:resource="https://iclg.com/practice-areas/public-investment-funds-laws-and-regulations/france"/>
		<rdfs:seeAlso rdf:resource="https://www.alfi.lu/en-gb/understandinginvesting/post/which-structure-to-choose"/>
		<rdfs:seeAlso rdf:resource="https://www.ubp.com/en/glossary-risk-management/glossary-legal-compliance/fcp"/>
		<skos:definition xml:lang="en">open-ended collective investment fund, which is a contractual form set up between the fund manager and investors and not a separate legal entity</skos:definition>
		<skos:note xml:lang="en">An FCP is similar to a unit trust in the UK. FCPs are not investment companies, but more like open partnerships. They can be set up as a single fund or as an umbrella fund with multiple sub-funds, typically issued in the French-speaking countries of Europe.</skos:note>
		<cmns-av:abbreviation xml:lang="en">FCP</cmns-av:abbreviation>
	</owl:Class>
	
	<owl:Class rdf:about="&fibo-sec-fund-civ;FundAccountant">
		<rdfs:subClassOf rdf:resource="&fibo-sec-fund-civ;FundsProcessingParty"/>
		<rdfs:label xml:lang="en">fund accountant</rdfs:label>
		<skos:definition xml:lang="en">The party that keeps accounting records of the available assets and liabilities of the Fund. It calculates dealing prices, the Net Asset Value (NAV) of the Fund, and may provide fund performance and tax data. Can be subcontracted by the FundAdministrator.</skos:definition>
	</owl:Class>
	
	<owl:Class rdf:about="&fibo-sec-fund-civ;FundAdministrator">
		<rdfs:subClassOf rdf:resource="&fibo-sec-fund-civ;FundsProcessingParty"/>
		<rdfs:subClassOf>
			<owl:Restriction>
				<owl:onProperty rdf:resource="&fibo-sec-fund-civ;mayAlsoBe"/>
				<owl:someValuesFrom rdf:resource="&fibo-sec-fund-civ;UnitIssuer"/>
			</owl:Restriction>
		</rdfs:subClassOf>
		<rdfs:subClassOf>
			<owl:Restriction>
				<owl:onProperty rdf:resource="&cmns-rlcmp;isPlayedBy"/>
				<owl:someValuesFrom rdf:resource="&cmns-org;LegalEntity"/>
			</owl:Restriction>
		</rdfs:subClassOf>
		<rdfs:label xml:lang="en">fund administrator</rdfs:label>
		<skos:definition xml:lang="en">Entity that has to fulfil the legal and supervisory requirements of the fund. Responsible for all the business purposes around the investment pool, and so is reponsible for the issuing of the shares.</skos:definition>
		<cmns-av:explanatoryNote xml:lang="en">If the unit is a bond, then the issuer is separate from the Fund Administrator. WG11 text: The party in charge of financial accounting, NAV calculation, management and performance fee calculation. Can also be in charge of orders centralisation and registration. Definition origin:EFAMA DD</cmns-av:explanatoryNote>
	</owl:Class>
	
	<owl:Class rdf:about="&fibo-sec-fund-civ;FundAuditor">
		<rdfs:subClassOf rdf:resource="&fibo-sec-fund-civ;FundsProcessingParty"/>
		<rdfs:label xml:lang="en">fund auditor</rdfs:label>
		<skos:definition xml:lang="en">The party that is in charge of examining and verifying a fund&apos;s financial and accounting records as well as supporting documents and fulfilment of legal requirements. Definition origin:EFAMA DD</skos:definition>
	</owl:Class>
	
	<owl:Class rdf:about="&fibo-sec-fund-civ;FundBondClassUnit">
		<rdfs:subClassOf rdf:resource="&fibo-sec-fund-fund;FundUnit"/>
		<rdfs:subClassOf>
			<owl:Restriction>
				<owl:onProperty rdf:resource="&fibo-fnd-gao-obj;hasStrategy"/>
				<owl:someValuesFrom rdf:resource="&fibo-sec-fund-civ;FundUnitDistributionPolicy"/>
			</owl:Restriction>
		</rdfs:subClassOf>
		<rdfs:subClassOf>
			<owl:Restriction>
				<owl:onProperty rdf:resource="&fibo-sec-fund-civ;hasExpectedCoupon"/>
				<owl:someValuesFrom rdf:resource="&fibo-sec-fund-civ;FundBondUnitCoupon"/>
			</owl:Restriction>
		</rdfs:subClassOf>
		<rdfs:label xml:lang="en">fund bond class unit</rdfs:label>
		<skos:definition xml:lang="en">A fund unit which takes the form of debt in that fund.</skos:definition>
		<cmns-av:explanatoryNote xml:lang="en">From EFAMA Review: called denominations e.g. issued in $5000 pieces. You cannot buy fractional amounts in a bond.</cmns-av:explanatoryNote>
	</owl:Class>
	
	<owl:Class rdf:about="&fibo-sec-fund-civ;FundBondUnitCoupon">
		<rdfs:subClassOf rdf:resource="&fibo-fnd-acc-cur;InterestRate"/>
		<rdfs:subClassOf>
			<owl:Restriction>
				<owl:onProperty rdf:resource="&fibo-sec-fund-civ;hasPolicyTerms"/>
				<owl:someValuesFrom rdf:resource="&fibo-sec-fund-civ;FundCouponPolicy"/>
			</owl:Restriction>
		</rdfs:subClassOf>
		<rdfs:label xml:lang="en">fund bond unit coupon</rdfs:label>
		<skos:definition xml:lang="en">A fixed coupon paid out to holders of the Fund Bond Unit.</skos:definition>
	</owl:Class>
	
	<owl:Class rdf:about="&fibo-sec-fund-civ;FundCashDistributionPolicy">
		<rdfs:subClassOf rdf:resource="&fibo-sec-fund-civ;FundUnitDistributionPolicy"/>
		<rdfs:label xml:lang="en">fund cash distribution policy</rdfs:label>
		<skos:definition xml:lang="en">Policy for distribution of cash dividends or notes in the event that the fund units have a distribution policy of &quot;Cash&quot; rather than &quot;Reinvestment&quot;.</skos:definition>
	</owl:Class>
	
	<owl:Class rdf:about="&fibo-sec-fund-civ;FundClassification">
		<rdfs:subClassOf rdf:resource="&cmns-cls;Classifier"/>
		<rdfs:subClassOf>
			<owl:Restriction>
				<owl:onProperty rdf:resource="&cmns-cls;classifies"/>
				<owl:someValuesFrom rdf:resource="&fibo-sec-sec-pls;CollectiveInvestmentVehicle"/>
			</owl:Restriction>
		</rdfs:subClassOf>
		<rdfs:label xml:lang="en">fund classification</rdfs:label>
		<skos:definition xml:lang="en">The category of the fund according to the asset class. This is a published code by which the Fund is classified. Further notes: Could be EFCF codes. This is the way in which &quot;Type of fund&quot; is articulated.</skos:definition>
	</owl:Class>
	
	<owl:Class rdf:about="&fibo-sec-fund-civ;FundClassificationScheme">
		<rdfs:subClassOf rdf:resource="&cmns-cls;ClassificationScheme"/>
		<rdfs:subClassOf>
			<owl:Restriction>
				<owl:onProperty rdf:resource="&cmns-dsg;defines"/>
				<owl:someValuesFrom rdf:resource="&fibo-sec-fund-civ;FundClassification"/>
			</owl:Restriction>
		</rdfs:subClassOf>
		<rdfs:label xml:lang="en">fund classification scheme</rdfs:label>
		<skos:definition xml:lang="en">A published scheme for the category of a fund according to the asset class.</skos:definition>
	</owl:Class>
	
	<owl:Class rdf:about="&fibo-sec-fund-civ;FundCouponPolicy">
		<rdfs:subClassOf rdf:resource="&fibo-sec-fund-civ;FundCashDistributionPolicy"/>
		<rdfs:label xml:lang="en">fund coupon policy</rdfs:label>
		<skos:definition xml:lang="en">Terms for the expected distribution of bond unit coupons.</skos:definition>
	</owl:Class>
	
	<owl:Class rdf:about="&fibo-sec-fund-civ;FundDepositary">
		<rdfs:subClassOf rdf:resource="&fibo-sec-fund-civ;FundsProcessingParty"/>
		<rdfs:subClassOf>
			<owl:Restriction>
				<owl:onProperty rdf:resource="&fibo-sec-fund-civ;providesDepositaryServiceFor"/>
				<owl:someValuesFrom rdf:resource="&fibo-sec-fund-fund;FundUnit"/>
			</owl:Restriction>
		</rdfs:subClassOf>
		<rdfs:label xml:lang="en">fund depositary</rdfs:label>
		<skos:definition xml:lang="en">The party that holds and safeguards holdings owned by a fund. It is also responsible for compliance of the portfolio with legal ratios etc.</skos:definition>
		<cmns-av:explanatoryNote xml:lang="en">The depository may delegate custody to another entity (custodian). Definition origin:EFAMA DD</cmns-av:explanatoryNote>
	</owl:Class>
	
	<owl:Class rdf:about="&fibo-sec-fund-civ;FundDistributionPolicy">
		<rdfs:subClassOf rdf:resource="&fibo-fnd-law-lcap;Policy"/>
		<rdfs:label xml:lang="en">fund distribution policy</rdfs:label>
		<skos:definition xml:lang="en">policy indicating the overall strategy or limitations on distribution for the fund</skos:definition>
		<cmns-av:explanatoryNote xml:lang="en">Note that individual classes of Fund Unit also have specific distribution polcies as they effect that class of unit. This class is for terms with wording of the form: &quot; ... whether or not it is possible to hold shares ...&quot; for a given parameter.</cmns-av:explanatoryNote>
	</owl:Class>
	
	<owl:Class rdf:about="&fibo-sec-fund-civ;FundDistributor">
		<rdfs:subClassOf rdf:resource="&fibo-sec-fund-civ;FundsProcessingParty"/>
		<rdfs:label xml:lang="en">fund distributor</rdfs:label>
		<skos:definition xml:lang="en">an entity through which a fund may be bought by or for an investor. This may be on a discretionary or advisory basis, or as an execution-only service. Definition origin:EFAMA DD</skos:definition>
	</owl:Class>
	
	<owl:Class rdf:about="&fibo-sec-fund-civ;FundDividendPolicy">
		<rdfs:subClassOf rdf:resource="&fibo-sec-fund-civ;FundCashDistributionPolicy"/>
		<rdfs:label xml:lang="en">fund dividend policy</rdfs:label>
		<skos:definition xml:lang="en">Terms for the expected distributions of dividends.</skos:definition>
	</owl:Class>
	
	<owl:Class rdf:about="&fibo-sec-fund-civ;FundInvestmentObjective">
		<rdfs:subClassOf rdf:resource="&fibo-fnd-gao-obj;InvestmentObjective"/>
		<rdfs:subClassOf>
			<owl:Restriction>
				<owl:onProperty rdf:resource="&fibo-sec-fund-civ;hasIntendedRiskLevel"/>
				<owl:someValuesFrom rdf:resource="&fibo-sec-fund-civ;RiskLevel"/>
			</owl:Restriction>
		</rdfs:subClassOf>
		<rdfs:subClassOf>
			<owl:Restriction>
				<owl:onProperty rdf:resource="&fibo-sec-fund-civ;statedIn"/>
				<owl:someValuesFrom rdf:resource="&fibo-sec-fund-civ;FundProspectus"/>
			</owl:Restriction>
		</rdfs:subClassOf>
		<rdfs:label xml:lang="en">fund investment objective</rdfs:label>
		<skos:definition xml:lang="en">The aim of a Fund e.g outperfom a given benchmark.</skos:definition>
		<skos:editorialNote xml:lang="en">This could be broken down into other terms that can be itemised here, that are not in the EFAMA DD explicitly. Examples may include: - Risk level - Return - Exposure to different markets</skos:editorialNote>
	</owl:Class>
	
	<owl:Class rdf:about="&fibo-sec-fund-civ;FundInvestmentPolicy">
		<rdfs:subClassOf rdf:resource="&fibo-fnd-law-lcap;Policy"/>
		<rdfs:subClassOf>
			<owl:Restriction>
				<owl:onProperty rdf:resource="&fibo-sec-fund-civ;stipulatesBenchmark"/>
				<owl:onClass rdf:resource="&fibo-ind-ind-ind;MarketRate"/>
				<owl:maxQualifiedCardinality rdf:datatype="&xsd;nonNegativeInteger">1</owl:maxQualifiedCardinality>
			</owl:Restriction>
		</rdfs:subClassOf>
		<rdfs:subClassOf>
			<owl:Restriction>
				<owl:onProperty rdf:resource="&cmns-dsg;defines"/>
				<owl:someValuesFrom rdf:resource="&fibo-sec-fund-civ;InvestmentRestriction"/>
			</owl:Restriction>
		</rdfs:subClassOf>
		<rdfs:subClassOf>
			<owl:Restriction>
				<owl:onProperty rdf:resource="&cmns-rga;governs"/>
				<owl:someValuesFrom rdf:resource="&fibo-sec-fund-civ;PortfolioInvestmentStrategy"/>
			</owl:Restriction>
		</rdfs:subClassOf>
		<rdfs:label xml:lang="en">fund investment policy</rdfs:label>
		<skos:definition xml:lang="en">policy that the fund implements in order to achieve the stated fund objectives</skos:definition>
		<cmns-av:explanatoryNote xml:lang="en">EFAMA Note: Model distinguishes between strategy (what you intend to invest in) and portfolio structure (what is held). This semantics matches the EFAMA DD &quot;Fund Investment Policy&quot; No stated definition in EFAMA DD (&quot;Further discussion required&quot;).</cmns-av:explanatoryNote>
	</owl:Class>
	
	<owl:Class rdf:about="&fibo-sec-fund-civ;FundLegalFormDocumentation">
		<rdfs:subClassOf rdf:resource="&fibo-fnd-law-cor;Constitution"/>
		<rdfs:label xml:lang="en">fund legal form documentation</rdfs:label>
		<skos:definition xml:lang="en">For a fund which is constituted under the law of contract, the constitution or articles that define the fund. These are embodied in a Contract.</skos:definition>
		<cmns-av:explanatoryNote xml:lang="en">From ISO FIBIM &quot;Umbrella Fund&quot; narrative: In securities, a collective investment scheme that has a contractual or a corporate form. When it has a contractual form, a fund is constituted under either the law of contract or under the trust law and thus it is not a legal entity. In its corporate form, a fund is a legal entity and is structured as a company.</cmns-av:explanatoryNote>
	</owl:Class>
	
	<owl:Class rdf:about="&fibo-sec-fund-civ;FundManagementCompany">
		<rdfs:subClassOf rdf:resource="&cmns-org;LegalEntity"/>
		<rdfs:label xml:lang="en">fund management company</rdfs:label>
		<skos:definition xml:lang="en">The party that sets up the fund, decides the investment strategy, appoints the agents, and is responsible for the promotion and the marketing of the fund. It makes all of the important decisions related to the fund. Also called fund promotor or fund sponsor or fund manager.</skos:definition>
		<cmns-av:explanatoryNote xml:lang="en">In the US: operates on a percentage of the Portfolio assets under management.</cmns-av:explanatoryNote>
	</owl:Class>
	
	<owl:Class rdf:about="&fibo-sec-fund-civ;FundManager">
		<rdfs:subClassOf rdf:resource="&fibo-sec-fund-civ;FundsProcessingParty"/>
		<rdfs:subClassOf>
			<owl:Restriction>
				<owl:onProperty rdf:resource="&cmns-rlcmp;isPlayedBy"/>
				<owl:someValuesFrom rdf:resource="&fibo-sec-fund-civ;FundManagementCompany"/>
			</owl:Restriction>
		</rdfs:subClassOf>
		<rdfs:label xml:lang="en">fund manager</rdfs:label>
		<skos:definition xml:lang="en">The party that sets up the fund, decides the investment strategy, appoints the agents, and is responsible for the promotion and the marketing of the fund. It makes all of the important decisions related to the fund. Also called fund promotor or fund sponsor. This is a dupliucate of Fund Management Company at the moment</skos:definition>
	</owl:Class>
	
	<owl:Class rdf:about="&fibo-sec-fund-civ;FundOrderDesk">
		<rdfs:subClassOf rdf:resource="&fibo-fbc-pas-caa;AccountProvider"/>
		<rdfs:subClassOf>
			<owl:Restriction>
				<owl:onProperty rdf:resource="&cmns-rlcmp;isPlayedBy"/>
				<owl:someValuesFrom rdf:resource="&cmns-org;LegalEntity"/>
			</owl:Restriction>
		</rdfs:subClassOf>
		<rdfs:label xml:lang="en">fund order desk</rdfs:label>
		<skos:definition xml:lang="en">The Fund Order Desk is a party to the Fund Order Desk Account.</skos:definition>
		<skos:editorialNote xml:lang="en">This party would presumably be identified as the Fund Management Company in terms of what legal entity fulcils this role? to be determined at further review.</skos:editorialNote>
	</owl:Class>
	
	<owl:Class rdf:about="&fibo-sec-fund-civ;FundPortfolio">
		<rdfs:subClassOf rdf:resource="&fibo-sec-sec-ast;Portfolio"/>
		<rdfs:subClassOf>
			<owl:Restriction>
				<owl:onProperty rdf:resource="&fibo-fnd-acc-cur;hasMonetaryAmount"/>
				<owl:someValuesFrom rdf:resource="&fibo-fbc-pas-caa;Balance"/>
			</owl:Restriction>
		</rdfs:subClassOf>
		<rdfs:subClassOf>
			<owl:Restriction>
				<owl:onProperty rdf:resource="&fibo-sec-fund-civ;assessedAgainst"/>
				<owl:someValuesFrom rdf:resource="&fibo-sec-fund-civ;PortfolioBenchmark"/>
			</owl:Restriction>
		</rdfs:subClassOf>
		<rdfs:subClassOf>
			<owl:Restriction>
				<owl:onProperty rdf:resource="&fibo-sec-fund-civ;hasInvestmentStrategy"/>
				<owl:someValuesFrom rdf:resource="&fibo-sec-fund-civ;PortfolioInvestmentStrategy"/>
			</owl:Restriction>
		</rdfs:subClassOf>
		<rdfs:subClassOf>
			<owl:Restriction>
				<owl:onProperty rdf:resource="&fibo-sec-fund-civ;hasLiquidity"/>
				<owl:someValuesFrom rdf:resource="&fibo-sec-fund-civ;Liquidity"/>
			</owl:Restriction>
		</rdfs:subClassOf>
		<rdfs:subClassOf>
			<owl:Restriction>
				<owl:onProperty rdf:resource="&fibo-sec-fund-civ;implementsFundPolicy"/>
				<owl:someValuesFrom rdf:resource="&fibo-sec-fund-civ;FundPortfolioInvestmentPolicy"/>
			</owl:Restriction>
		</rdfs:subClassOf>
		<rdfs:subClassOf>
			<owl:Restriction>
				<owl:onProperty rdf:resource="&cmns-col;comprises"/>
				<owl:someValuesFrom rdf:resource="&fibo-sec-sec-ast;Portfolio"/>
			</owl:Restriction>
		</rdfs:subClassOf>
		<rdfs:subClassOf>
			<owl:Restriction>
				<owl:onProperty rdf:resource="&cmns-org;isManagedBy"/>
				<owl:someValuesFrom rdf:resource="&fibo-sec-fund-civ;PortfolioManager"/>
			</owl:Restriction>
		</rdfs:subClassOf>
		<rdfs:label xml:lang="en">fund portfolio</rdfs:label>
		<skos:definition xml:lang="en">An account containing a number of financial instruments along with cash positions in one or more currencies and belonging to a Fund</skos:definition>
	</owl:Class>
	
	<owl:Class rdf:about="&fibo-sec-fund-civ;FundPortfolioInvestmentLimitations">
		<rdfs:subClassOf rdf:resource="&fibo-sec-fund-civ;InvestmentRestriction"/>
		<rdfs:label xml:lang="en">fund portfolio investment limitations</rdfs:label>
		<skos:definition xml:lang="en">Detailed Policy on approximately how the portfolio is to be allocated to achieve the stated investment goals. This underpins the detailed strategy of how to achieve this.</skos:definition>
		<cmns-av:explanatoryNote xml:lang="en">Defined as &quot;Strategy&quot; in FIBIM and elsewhere. WG11: Rough allocation of the portfolio.</cmns-av:explanatoryNote>
	</owl:Class>
	
	<owl:Class rdf:about="&fibo-sec-fund-civ;FundPortfolioInvestmentPolicy">
		<rdfs:subClassOf rdf:resource="&fibo-fnd-law-lcap;Policy"/>
		<rdfs:subClassOf>
			<owl:Restriction>
				<owl:onProperty rdf:resource="&fibo-sec-fund-civ;definesAllocations"/>
				<owl:someValuesFrom rdf:resource="&fibo-sec-fund-civ;FundPortfolioInvestmentLimitations"/>
			</owl:Restriction>
		</rdfs:subClassOf>
		<rdfs:subClassOf>
			<owl:Restriction>
				<owl:onProperty rdf:resource="&cmns-rga;governs"/>
				<owl:someValuesFrom rdf:resource="&fibo-sec-fund-civ;PortfolioInvestmentStrategy"/>
			</owl:Restriction>
		</rdfs:subClassOf>
		<rdfs:label xml:lang="en">fund portfolio investment policy</rdfs:label>
		<skos:definition xml:lang="en">policy with respect to allocation of the portfolio that is designed to meet the stated investment strategy and goals</skos:definition>
		<cmns-av:explanatoryNote xml:lang="en">ISO FIBIM: Rough allocation of the portfolio.</cmns-av:explanatoryNote>
	</owl:Class>
	
	<owl:Class rdf:about="&fibo-sec-fund-civ;FundProcessingGeneralTerms">
		<rdfs:subClassOf rdf:resource="&fibo-sec-fund-civ;FundProcessingTerms"/>
		<rdfs:label xml:lang="en">fund processing general terms</rdfs:label>
		<skos:definition xml:lang="en">Formal terms for general processing of the fund. These set out what the investor and the fund may or may not do.</skos:definition>
	</owl:Class>
	
	<owl:Class rdf:about="&fibo-sec-fund-civ;FundProcessingTerms">
		<rdfs:subClassOf rdf:resource="&fibo-fnd-agr-ctr;ContractualCommitment"/>
		<rdfs:subClassOf>
			<owl:Restriction>
				<owl:onProperty rdf:resource="&fibo-sec-fund-civ;definesMainFundOrderDeskAccount"/>
				<owl:someValuesFrom rdf:resource="&fibo-sec-fund-civ;FundsProcessingAccount"/>
			</owl:Restriction>
		</rdfs:subClassOf>
		<rdfs:subClassOf>
			<owl:Restriction>
				<owl:onProperty rdf:resource="&fibo-sec-fund-civ;hasDefaultSettlementConvention"/>
				<owl:someValuesFrom rdf:resource="&fibo-fbc-fi-stl;SettlementConvention"/>
			</owl:Restriction>
		</rdfs:subClassOf>
		<rdfs:label xml:lang="en">fund processing terms</rdfs:label>
		<skos:definition xml:lang="en">Formal terms for processing of the fund. These set out what the investor and the fund may or may not do. These include terms for redemption and subscription processing as well as general processing terms. ISO FIBIM definition: Processing characteristics linked to the instrument, ie, not to the market.</skos:definition>
		<cmns-av:explanatoryNote xml:lang="en">These include Fund Subscription Terms, Fund Redemption Terms. and terms which relate to general processing and restrictions or otherwise on the holder. FPP notes: FPP presentation identifies many of these terms under the heading of Valuation Dealing characteristics. May need to revise which goes where in line with FPP. See also terms under NAV Valuation Calculation Method. Others of these terms appear in FPP under Instrument Restrictions. These cover the subscription, redemption and holding amounts and units and minimum holding period.</cmns-av:explanatoryNote>
	</owl:Class>
	
	<owl:Class rdf:about="&fibo-sec-fund-civ;FundPromoter">
		<rdfs:subClassOf rdf:resource="&fibo-sec-fund-civ;FundsProcessingParty"/>
		<rdfs:label xml:lang="en">fund promoter</rdfs:label>
		<skos:definition xml:lang="en">An entity that promotes a fund. May be an investor, pension fund, bank, insurance company or management company</skos:definition>
	</owl:Class>
	
	<owl:Class rdf:about="&fibo-sec-fund-civ;FundProspectus">
		<rdfs:subClassOf rdf:resource="&fibo-sec-sec-iss;Prospectus"/>
		<rdfs:subClassOf>
			<owl:Restriction>
				<owl:onProperty rdf:resource="&fibo-sec-fund-civ;anticipates"/>
				<owl:someValuesFrom rdf:resource="&fibo-ind-ind-ind;MarketRate"/>
			</owl:Restriction>
		</rdfs:subClassOf>
		<rdfs:subClassOf>
			<owl:Restriction>
				<owl:onProperty rdf:resource="&fibo-sec-fund-civ;outlines"/>
				<owl:someValuesFrom rdf:resource="&fibo-sec-fund-civ;FundInvestmentObjective"/>
			</owl:Restriction>
		</rdfs:subClassOf>
		<rdfs:label xml:lang="en">fund prospectus</rdfs:label>
		<skos:definition xml:lang="en">The Prospectus for the Fund. This is a document made available publicly for potential investors. It will include facts about the fund investment objective, investment focus and other details of the fund. Some of this information becomes binding on the fund once it is issued, while other information is guidelines only.</skos:definition>
		<skos:editorialNote xml:lang="en">EFAMA Review description for this: The fund is issued with a prospectus; there is material in the prospectus that is binding; material that is expected but not binding, and information that may or may not be in the prospectus or a given fund.</skos:editorialNote>
	</owl:Class>
	
	<owl:Class rdf:about="&fibo-sec-fund-civ;FundRedemptionRestriction">
		<rdfs:subClassOf rdf:resource="&fibo-sec-sec-rst;SecuritiesRestriction"/>
		<rdfs:label xml:lang="en">fund redemption restriction</rdfs:label>
	</owl:Class>
	
	<owl:Class rdf:about="&fibo-sec-fund-civ;FundRedemptionTerms">
		<rdfs:subClassOf rdf:resource="&fibo-sec-fund-civ;FundProcessingTerms"/>
		<rdfs:subClassOf>
			<owl:Restriction>
				<owl:onProperty rdf:resource="&fibo-sec-fund-civ;hasAdditionalRedemptionRestrictions"/>
				<owl:someValuesFrom rdf:resource="&fibo-sec-fund-civ;ReferToFundOrderDesk"/>
			</owl:Restriction>
		</rdfs:subClassOf>
		<rdfs:label xml:lang="en">fund redemption terms</rdfs:label>
		<skos:definition xml:lang="en">Formal terms for redemption of units in the fund. These set out what the investor and the fund may or may not do.</skos:definition>
	</owl:Class>
	
	<owl:Class rdf:about="&fibo-sec-fund-civ;FundReinvestmentPolicy">
		<rdfs:subClassOf rdf:resource="&fibo-sec-fund-civ;FundUnitDistributionPolicy"/>
		<rdfs:label xml:lang="en">fund reinvestment policy</rdfs:label>
		<skos:definition xml:lang="en">Terms for the expected reinvestment of profits on fund units.</skos:definition>
	</owl:Class>
	
	<owl:Class rdf:about="&fibo-sec-fund-civ;FundShareClassUnit">
		<rdfs:subClassOf rdf:resource="&fibo-sec-fund-fund;FundUnit"/>
		<rdfs:subClassOf>
			<owl:Restriction>
				<owl:onProperty rdf:resource="&fibo-fnd-gao-obj;hasStrategy"/>
				<owl:someValuesFrom rdf:resource="&fibo-sec-fund-civ;FundUnitDistributionPolicy"/>
			</owl:Restriction>
		</rdfs:subClassOf>
		<rdfs:label xml:lang="en">fund share class unit</rdfs:label>
		<skos:definition xml:lang="en">The legal structure in which you can purchase part of an investment pool, defined by a variety of characteristics like investor type, minimum size of investment, distribution type, fee and currency. A fund unit which gives the holder an equity stake in the fund.</skos:definition>
		<cmns-av:explanatoryNote xml:lang="en">From review sessions: Theoretically you can buy a fraction of a share in a fund. This would depend on the legal structure of the fund, e.g. a minimum investment. There is always a distribution plan.</cmns-av:explanatoryNote>
	</owl:Class>
	
	<owl:Class rdf:about="&fibo-sec-fund-civ;FundSubscriptionTerms">
		<rdfs:subClassOf rdf:resource="&fibo-sec-fund-civ;FundProcessingTerms"/>
		<rdfs:subClassOf>
			<owl:Restriction>
				<owl:onProperty rdf:resource="&cmns-cxtdsg;appliesTo"/>
				<owl:someValuesFrom rdf:resource="&fibo-sec-fund-fund;FundUnit"/>
			</owl:Restriction>
		</rdfs:subClassOf>
		<rdfs:label xml:lang="en">fund subscription terms</rdfs:label>
		<skos:definition xml:lang="en">Subscription terms for the fund. Further notes: ISO FIBIM, EFAMA DD and FPP combine terms for subscription, redemption and general holding requirements. These have been separated here as they are different kinds of term, but this can be reviewed. Subscription Terms are identified as terms of the fund and not the fund unit, since terms for how you might subscribe can&apos;t be binding one someone who has not yet subscribed.</skos:definition>
	</owl:Class>
	
	<owl:Class rdf:about="&fibo-sec-fund-civ;FundSupervisoryAuthority">
		<rdfs:subClassOf rdf:resource="&cmns-pts;PartyRole"/>
		<rdfs:label xml:lang="en">fund supervisory authority</rdfs:label>
		<skos:definition xml:lang="en">party that supervises the fund or fund industry</skos:definition>
	</owl:Class>
	
	<owl:Class rdf:about="&fibo-sec-fund-civ;FundTransferAgent">
		<rdfs:subClassOf rdf:resource="&fibo-sec-fund-civ;FundsProcessingParty"/>
		<rdfs:label xml:lang="en">fund transfer agent</rdfs:label>
		<skos:definition xml:lang="en">An entity that undertakes the execution of subscription, redemption and switch orders on behalf of a fund. Definition origin:EFAMA DD</skos:definition>
	</owl:Class>
	
	<owl:Class rdf:about="&fibo-sec-fund-civ;FundUnitDistributionMethod">
		<rdfs:subClassOf rdf:resource="&fibo-fnd-gao-obj;DistributionStrategy"/>
		<rdfs:label xml:lang="en">fund unit distribution method</rdfs:label>
		<skos:definition xml:lang="en">The normal distribution policy for funds.</skos:definition>
	</owl:Class>
	
	<owl:Class rdf:about="&fibo-sec-fund-civ;FundUnitDistributionPolicy">
		<rdfs:subClassOf rdf:resource="&fibo-fnd-law-lcap;Policy"/>
		<rdfs:subClassOf>
			<owl:Restriction>
				<owl:onProperty rdf:resource="&fibo-fnd-gao-obj;hasStrategy"/>
				<owl:someValuesFrom rdf:resource="&fibo-sec-fund-civ;FundUnitDistributionMethod"/>
			</owl:Restriction>
		</rdfs:subClassOf>
		<rdfs:label xml:lang="en">fund unit distribution policy</rdfs:label>
		<skos:definition xml:lang="en">policy relating to the unit, e.g. if income is paid out or retained in the fund and how this is treated, including distribution policy details for dividends and coupons.</skos:definition>
	</owl:Class>
	
	<owl:Class rdf:about="&fibo-sec-fund-civ;FundUnitHolding">
		<rdfs:subClassOf rdf:resource="&fibo-sec-sec-ast;Portfolio"/>
		<rdfs:subClassOf>
			<owl:Restriction>
				<owl:onProperty rdf:resource="&cmns-col;comprises"/>
				<owl:allValuesFrom rdf:resource="&fibo-sec-fund-fund;FundUnit"/>
			</owl:Restriction>
		</rdfs:subClassOf>
		<rdfs:label xml:lang="en">fund unit holding</rdfs:label>
		<skos:definition xml:lang="en">A holding of a unit in another fund.</skos:definition>
	</owl:Class>
	
	<owl:Class rdf:about="&fibo-sec-fund-civ;FundsCashDistribution">
		<rdfs:subClassOf rdf:resource="&fibo-sec-fund-civ;FundUnitDistributionMethod"/>
		<rdfs:label xml:lang="en">funds cash distribution</rdfs:label>
		<skos:definition xml:lang="en">Accrued income is distributed periodically to the investor.</skos:definition>
	</owl:Class>
	
	<owl:Class rdf:about="&fibo-sec-fund-civ;FundsProcessing">
		<rdfs:subClassOf rdf:resource="&fibo-fnd-arr-lif;LifecycleStage"/>
		<rdfs:label xml:lang="en">funds processing</rdfs:label>
		<skos:definition xml:lang="en">The context of managing and processing funds, issuing funds units etc. This is the context in which the different parties involved in a fund are defined as parties.</skos:definition>
	</owl:Class>
	
	<owl:Class rdf:about="&fibo-sec-fund-civ;FundsProcessingAccount">
		<rdfs:subClassOf rdf:resource="&fibo-fbc-pas-caa;Account"/>
		<rdfs:subClassOf>
			<owl:Restriction>
				<owl:onProperty rdf:resource="&cmns-org;isProvidedBy"/>
				<owl:someValuesFrom rdf:resource="&fibo-sec-fund-civ;FundOrderDesk"/>
			</owl:Restriction>
		</rdfs:subClassOf>
		<rdfs:label xml:lang="en">funds processing account</rdfs:label>
		<skos:definition xml:lang="en">An account used specifically in the processing of funds. Like all accounts this is (per FIBIM definition) a business relationship between two entities; one entity is the account owner, the other entity is the account servicer. Please refer to Financial global model for treatment of accounts relationships in this model.</skos:definition>
		<cmns-av:explanatoryNote xml:lang="en">Derived from FIBIM definition for &quot;Account&quot;, which is: &quot;Business relationship between two entities; one entity is the account owner, the other entity is the account servicer.&quot; this corresponds to the Global Terms definition for Account.</cmns-av:explanatoryNote>
	</owl:Class>
	
	<owl:Class rdf:about="&fibo-sec-fund-civ;FundsProcessingParty">
		<rdfs:subClassOf rdf:resource="&cmns-pts;PartyRole"/>
		<rdfs:label xml:lang="en">funds processing party</rdfs:label>
		<skos:definition xml:lang="en">party involved in the processing of funds</skos:definition>
	</owl:Class>
	
	<owl:Class rdf:about="&fibo-sec-fund-civ;IncomeAccumulation">
		<rdfs:subClassOf rdf:resource="&fibo-sec-fund-civ;FundUnitDistributionMethod"/>
		<rdfs:label xml:lang="en">income accumulation</rdfs:label>
		<skos:definition xml:lang="en">Accrued income is not distributed and instead remains reflected within the unit/share price.</skos:definition>
	</owl:Class>
	
	<owl:Class rdf:about="&fibo-sec-fund-civ;InvestmentAdvisor">
		<rdfs:subClassOf rdf:resource="&fibo-sec-fund-civ;FundsProcessingParty"/>
		<rdfs:subClassOf>
			<owl:Restriction>
				<owl:onProperty rdf:resource="&cmns-rlcmp;isPlayedBy"/>
				<owl:someValuesFrom rdf:resource="&cmns-org;LegalEntity"/>
			</owl:Restriction>
		</rdfs:subClassOf>
		<rdfs:label xml:lang="en">investment advisor</rdfs:label>
		<skos:definition xml:lang="en">The party that provides investment guidance at a fee. Definition origin:EFAMA DD</skos:definition>
	</owl:Class>
	
	<owl:Class rdf:about="&fibo-sec-fund-civ;InvestmentRestriction">
		<rdfs:subClassOf rdf:resource="&fibo-sec-sec-rst;SecuritiesRestriction"/>
		<rdfs:subClassOf>
			<owl:Restriction>
				<owl:onProperty rdf:resource="&cmns-col;isPartOf"/>
				<owl:someValuesFrom rdf:resource="&fibo-sec-fund-civ;FundProspectus"/>
			</owl:Restriction>
		</rdfs:subClassOf>
		<rdfs:label xml:lang="en">fund investment restrictions set</rdfs:label>
		<skos:definition xml:lang="en">Limitations that apply to the fund as a whole, such as risk factors. these are used to determine whether the fund is appropriate for a given type of investor to invest in.</skos:definition>
		<cmns-av:explanatoryNote xml:lang="en">These are defined by the overall Fund investment policy. Not the same as the detailed policies for investing in percentages of this or that.</cmns-av:explanatoryNote>
	</owl:Class>
	
	<owl:Class rdf:about="&fibo-sec-fund-civ;InvestmentStrategy">
		<rdfs:subClassOf rdf:resource="&fibo-fnd-gao-obj;BusinessStrategy"/>
		<rdfs:subClassOf>
			<owl:Restriction>
				<owl:onProperty rdf:resource="&fibo-fnd-gao-obj;hasObjective"/>
				<owl:someValuesFrom rdf:resource="&fibo-fnd-gao-obj;InvestmentObjective"/>
			</owl:Restriction>
		</rdfs:subClassOf>
		<rdfs:label xml:lang="en">investment strategy</rdfs:label>
		<skos:definition xml:lang="en">plan, method, or series of maneuvers or stratagems for obtaining a specific investment goal</skos:definition>
	</owl:Class>
	
	<owl:Class rdf:about="&fibo-sec-fund-civ;JurisdictionStrategy">
		<rdfs:subClassOf rdf:resource="&fibo-sec-fund-civ;FundPortfolioInvestmentLimitations"/>
		<rdfs:subClassOf>
			<owl:Restriction>
				<owl:onProperty rdf:resource="&cmns-cxtdsg;isApplicableIn"/>
				<owl:someValuesFrom rdf:resource="&cmns-rga;Jurisdiction"/>
			</owl:Restriction>
		</rdfs:subClassOf>
		<rdfs:label xml:lang="en">jurisdiction strategy</rdfs:label>
		<skos:definition xml:lang="en">Strategy which is jurisdiction based.</skos:definition>
	</owl:Class>
	
	<owl:Class rdf:about="&fibo-sec-fund-civ;KeyInvestorInformationDocument">
		<rdfs:subClassOf rdf:resource="&fibo-sec-sec-iss;OfferingDocument"/>
		<rdfs:subClassOf>
			<owl:Restriction>
				<owl:onProperty rdf:resource="&cmns-cxtdsg;isApplicableIn"/>
				<owl:hasValue rdf:resource="&fibo-be-ge-euj;EuropeanUnionJurisdiction"/>
			</owl:Restriction>
		</rdfs:subClassOf>
		<rdfs:subClassOf>
			<owl:Restriction>
				<owl:onProperty rdf:resource="&cmns-cxtdsg;appliesTo"/>
				<owl:someValuesFrom rdf:resource="&fibo-sec-fund-fund;FundUnit"/>
			</owl:Restriction>
		</rdfs:subClassOf>
		<rdfs:label>key investor information document</rdfs:label>
		<skos:definition>short document that provides critical information for investors, summarizing content derived from a prospectus such that it can be understood by investors without reference to other documents, as required by law in the European Union</skos:definition>
		<cmns-av:abbreviation>KIID</cmns-av:abbreviation>
		<cmns-av:adaptedFrom rdf:datatype="&xsd;anyURI">https://eur-lex.europa.eu/eli/dir/2009/65/2020-01-07</cmns-av:adaptedFrom>
		<cmns-av:explanatoryNote>Key investor information shall include appropriate information about the essential characteristics of the UCITS concerned, which is to be provided to investors so that they are reasonably able to understand the nature and the risks of the investment product that is being offered to them and, consequently, to take investment decisions on an informed basis.</cmns-av:explanatoryNote>
	</owl:Class>
	
	<owl:Class rdf:about="&fibo-sec-fund-civ;Liquidity">
		<rdfs:subClassOf rdf:resource="&fibo-fnd-oac-own;Asset"/>
		<rdfs:subClassOf>
			<owl:Restriction>
				<owl:onProperty rdf:resource="&fibo-fnd-acc-cur;hasCurrency"/>
				<owl:someValuesFrom rdf:resource="&fibo-fnd-acc-cur;Currency"/>
			</owl:Restriction>
		</rdfs:subClassOf>
		<rdfs:label xml:lang="en">liquidity</rdfs:label>
		<skos:definition xml:lang="en">Precise definition needed for liquidity, and check that it is modeled accordingly.</skos:definition>
	</owl:Class>
	
	<owl:Class rdf:about="&fibo-sec-fund-civ;NetAssetValueCalculationMethod">
		<rdfs:subClassOf rdf:resource="&cmns-qtu;Expression"/>
		<rdfs:subClassOf>
			<owl:Restriction>
				<owl:onProperty rdf:resource="&fibo-sec-fund-civ;isCalculatedIn"/>
				<owl:someValuesFrom rdf:resource="&fibo-fnd-acc-cur;Currency"/>
			</owl:Restriction>
		</rdfs:subClassOf>
		<rdfs:label xml:lang="en">net asset value calculation method</rdfs:label>
		<skos:definition xml:lang="en">Parameters for the calculation of the net asset value for an investment fund/fund class.</skos:definition>
		<skos:editorialNote xml:lang="en">These terms were in the ISO FIBIM model but correspond to some details in the EFAMA DD.</skos:editorialNote>
	</owl:Class>
	
	<owl:Class rdf:about="&fibo-sec-fund-civ;NoteFundUnit">
		<rdfs:subClassOf rdf:resource="&fibo-sec-fund-fund;FundUnit"/>
		<rdfs:label xml:lang="en">note fund unit</rdfs:label>
		<skos:definition xml:lang="en">Need a legal definition - to follow. This is one of the mechanisms by which an investor may hold an interest in a fund, but is not a Bond or a Share.</skos:definition>
		<skos:editorialNote xml:lang="en">It is not possible to determine at this time whether some of the policy facts that apply to bund and share class units apply to all fund units including this one. Once this is defined, all Fund Distribution Policy terms and relationships should be rechecked.</skos:editorialNote>
	</owl:Class>
	
	<owl:Class rdf:about="&fibo-sec-fund-civ;OrganizationStrategy">
		<rdfs:subClassOf rdf:resource="&fibo-sec-fund-civ;FundPortfolioInvestmentLimitations"/>
		<rdfs:subClassOf>
			<owl:Restriction>
				<owl:onProperty rdf:resource="&fibo-sec-fund-civ;definedInRelationTo"/>
				<owl:someValuesFrom rdf:resource="&fibo-be-le-cb;Corporation"/>
			</owl:Restriction>
		</rdfs:subClassOf>
		<rdfs:label xml:lang="en">organization strategy</rdfs:label>
		<skos:definition xml:lang="en">Strategy which is organization based.</skos:definition>
	</owl:Class>
	
	<owl:Class rdf:about="&fibo-sec-fund-civ;OtherInvestmentFundInformation">
		<rdfs:subClassOf rdf:resource="&cmns-doc;Document"/>
		<rdfs:label xml:lang="en">other investment fund information</rdfs:label>
		<skos:definition xml:lang="en">Things which are not part of the prospectus but are important if you want to understand the fund.</skos:definition>
		<skos:editorialNote xml:lang="en">See terms in EFAMA spreadsheet. These are properties of the fund but are not legally binding. Author follow-up note: I have managed to find a &quot;home&quot; for disposition for most of the entries that are in the spreadsheet. It is not clear which of the spreadsheet terms are indended to come under the general heading in this class. The first place I would look is in the terms I have defined as &quot;Fund Processing Terms&quot;, which are defined as formal, legal contractual terms. If any of those are not legally binding on some party, then this is where they belong instead.</skos:editorialNote>
	</owl:Class>
	
	<owl:Class rdf:about="&fibo-sec-fund-civ;PortfolioBenchmark">
		<rdfs:subClassOf rdf:resource="&cmns-qtu;Measure"/>
		<rdfs:subClassOf>
			<owl:Restriction>
				<owl:onProperty rdf:resource="&fibo-sec-fund-civ;definesBenchmark"/>
				<owl:someValuesFrom rdf:resource="&fibo-ind-ind-ind;MarketRate"/>
			</owl:Restriction>
		</rdfs:subClassOf>
		<rdfs:subClassOf>
			<owl:Restriction>
				<owl:onProperty rdf:resource="&cmns-cxtdsg;appliesTo"/>
				<owl:someValuesFrom rdf:resource="&fibo-sec-fund-civ;FundPortfolio"/>
			</owl:Restriction>
		</rdfs:subClassOf>
		<rdfs:label xml:lang="en">portfolio benchmark</rdfs:label>
		<skos:definition xml:lang="en">Security or other price against which the performance of the portfolio is evaluated.</skos:definition>
	</owl:Class>
	
	<owl:Class rdf:about="&fibo-sec-fund-civ;PortfolioInvestmentStrategy">
		<rdfs:subClassOf rdf:resource="&fibo-sec-fund-civ;InvestmentStrategy"/>
		<rdfs:subClassOf>
			<owl:Restriction>
				<owl:onProperty rdf:resource="&cmns-col;comprises"/>
				<owl:someValuesFrom rdf:resource="&fibo-sec-fund-civ;FundPortfolioInvestmentLimitations"/>
			</owl:Restriction>
		</rdfs:subClassOf>
		<rdfs:label xml:lang="en">portfolio investment strategy</rdfs:label>
		<skos:definition xml:lang="en">The manner in which the portfolio manager tries to reach the funds objectives.</skos:definition>
		<cmns-av:explanatoryNote xml:lang="en">Describes how you get there. E.g fully invested v not fully invested. MB Note: The terms labeled &quot;Strategy&quot; in EFAMA and in FIBIM are more like dictionary definition of policy, while &quot;How you get there&quot; is a dictionary definition of Strategy. Therefore original labels may be reversed from dictionary definition of the global semantics these are derived from.</cmns-av:explanatoryNote>
	</owl:Class>
	
	<owl:Class rdf:about="&fibo-sec-fund-civ;PortfolioManager">
		<rdfs:subClassOf rdf:resource="&cmns-org;OrganizationMember"/>
		<rdfs:subClassOf>
			<owl:Restriction>
				<owl:onProperty rdf:resource="&cmns-org;manages"/>
				<owl:someValuesFrom rdf:resource="&fibo-sec-fund-civ;FundPortfolio"/>
			</owl:Restriction>
		</rdfs:subClassOf>
		<rdfs:subClassOf>
			<owl:Restriction>
				<owl:onProperty rdf:resource="&cmns-rlcmp;isPlayedBy"/>
				<owl:someValuesFrom>
					<owl:Restriction>
						<owl:onProperty rdf:resource="&cmns-col;isMemberOf"/>
						<owl:allValuesFrom rdf:resource="&fibo-sec-fund-civ;FundManagementCompany"/>
					</owl:Restriction>
				</owl:someValuesFrom>
			</owl:Restriction>
		</rdfs:subClassOf>
		<rdfs:label>portfolio manager</rdfs:label>
		<skos:definition>person or entity responsible for day to day investment decisions for a fund or asset</skos:definition>
	</owl:Class>
	
	<owl:Class rdf:about="&fibo-sec-fund-civ;PreferredShareInFund">
		<rdfs:subClassOf rdf:resource="&fibo-sec-fund-civ;FundShareClassUnit"/>
		<rdfs:label xml:lang="en">preferred share in fund</rdfs:label>
	</owl:Class>
	
	<owl:Class rdf:about="&fibo-sec-fund-civ;PrivateEquityHolding">
		<rdfs:subClassOf rdf:resource="&fibo-sec-sec-ast;Portfolio"/>
		<rdfs:subClassOf>
			<owl:Restriction>
				<owl:onProperty rdf:resource="&cmns-col;comprises"/>
				<owl:someValuesFrom rdf:resource="&fibo-sec-eq-eq;PrivatelyHeldShare"/>
			</owl:Restriction>
		</rdfs:subClassOf>
		<rdfs:label xml:lang="en">private equity holding</rdfs:label>
		<skos:definition xml:lang="en">A holding of private equity.</skos:definition>
	</owl:Class>
	
	<owl:Class rdf:about="&fibo-sec-fund-civ;RealEstateHolding">
		<rdfs:subClassOf rdf:resource="&fibo-sec-sec-ast;Portfolio"/>
		<rdfs:subClassOf>
			<owl:Restriction>
				<owl:onProperty rdf:resource="&cmns-col;comprises"/>
				<owl:someValuesFrom rdf:resource="&fibo-fnd-plc-rp;RealEstate"/>
			</owl:Restriction>
		</rdfs:subClassOf>
		<rdfs:label xml:lang="en">real estate holding</rdfs:label>
		<skos:definition xml:lang="en">tangible asset consisting of real estate that is owned or controlled by an individual, organization, or entity for investment, operational, or strategic purposes</skos:definition>
	</owl:Class>
	
	<owl:Class rdf:about="&fibo-sec-fund-civ;ReferToFundOrderDesk">
		<rdfs:subClassOf rdf:resource="&fibo-sec-fund-civ;FundRedemptionRestriction"/>
		<rdfs:label xml:lang="en">refer to fund order desk</rdfs:label>
		<skos:definition xml:lang="en">Restriction requiring an investor to refer to the fund order desk prior to redeeming a fund.</skos:definition>
		<skos:editorialNote xml:lang="en">While it&apos;s unclear from original data models, it&apos;s likely that this restriction is actually to learn from the fund order desk of any other individual kinds of restriction that will apply. This is itself treated as a kind of restriction here.</skos:editorialNote>
	</owl:Class>
	
	<owl:Class rdf:about="&fibo-sec-fund-civ;RiskLevel">
		<rdfs:subClassOf rdf:resource="&cmns-cls;Classifier"/>
		<rdfs:label xml:lang="en">risk level</rdfs:label>
	</owl:Class>
	
	<owl:Class rdf:about="&fibo-sec-fund-civ;SICAF">
		<rdfs:subClassOf rdf:resource="&fibo-sec-sec-pls;CollectiveInvestmentVehicle"/>
		<rdfs:label xml:lang="en">s i c a f</rdfs:label>
		<skos:definition xml:lang="en">A French fund vehicle type. Designation and definition needed.</skos:definition>
	</owl:Class>
	
	<owl:Class rdf:about="&fibo-sec-fund-civ;SICAV">
		<rdfs:subClassOf rdf:resource="&fibo-sec-sec-pls;CollectiveInvestmentVehicle"/>
		<rdfs:label xml:lang="en">s i c a v</rdfs:label>
		<skos:definition xml:lang="en">Societe Collective a Capital Variable</skos:definition>
	</owl:Class>
	
	<owl:Class rdf:about="&fibo-sec-fund-civ;SectorStrategy">
		<rdfs:subClassOf rdf:resource="&fibo-sec-fund-civ;FundPortfolioInvestmentLimitations"/>
		<rdfs:label xml:lang="en">sector strategy</rdfs:label>
		<skos:definition xml:lang="en">Strategy which is sector based.</skos:definition>
	</owl:Class>
	
	<owl:Class rdf:about="&fibo-sec-fund-civ;StakeInFund">
		<rdfs:subClassOf rdf:resource="&fibo-fbc-pas-fpas;Position"/>
		<rdfs:subClassOf>
			<owl:Restriction>
				<owl:onProperty rdf:resource="&fibo-sec-fund-civ;givesOwnershipOf"/>
				<owl:someValuesFrom rdf:resource="&fibo-sec-sec-pls;CollectiveInvestmentVehicle"/>
			</owl:Restriction>
		</rdfs:subClassOf>
		<rdfs:subClassOf>
			<owl:Restriction>
				<owl:onProperty rdf:resource="&cmns-doc;refersTo"/>
				<owl:someValuesFrom rdf:resource="&fibo-sec-fund-fund;FundUnit"/>
			</owl:Restriction>
		</rdfs:subClassOf>
		<rdfs:label xml:lang="en">stake in fund</rdfs:label>
		<skos:definition xml:lang="en">The holding of some portion in a fund, by some party. This stake will generally tak ethe form of some sort of unit in that fund.</skos:definition>
	</owl:Class>
	
	<owl:Class rdf:about="&fibo-sec-fund-civ;UnitIssuer">
		<rdfs:subClassOf rdf:resource="&fibo-sec-fund-civ;FundsProcessingParty"/>
		<rdfs:subClassOf>
			<owl:Restriction>
				<owl:onProperty rdf:resource="&fibo-fnd-rel-rel;issues"/>
				<owl:someValuesFrom rdf:resource="&fibo-sec-fund-fund;FundUnit"/>
			</owl:Restriction>
		</rdfs:subClassOf>
		<rdfs:subClassOf>
			<owl:Restriction>
				<owl:onProperty rdf:resource="&cmns-rlcmp;isPlayedBy"/>
				<owl:someValuesFrom rdf:resource="&fibo-be-le-cb;Corporation"/>
			</owl:Restriction>
		</rdfs:subClassOf>
		<rdfs:label xml:lang="en">unit issuer</rdfs:label>
		<skos:definition xml:lang="en">The party which issues the Fund Unit.</skos:definition>
	</owl:Class>
	
	<owl:ObjectProperty rdf:about="&fibo-sec-fund-civ;accountingYearEndDate">
		<rdfs:label xml:lang="en">accounting year end date</rdfs:label>
		<rdfs:range rdf:resource="&fibo-fnd-dt-bd;DayOfMonth"/>
		<skos:definition xml:lang="en">Last day of the accounting year for the fund.</skos:definition>
	</owl:ObjectProperty>
	
	<owl:DatatypeProperty rdf:about="&fibo-sec-fund-civ;additionalRestrictions">
		<rdfs:label xml:lang="en">additional restrictions</rdfs:label>
		<rdfs:domain rdf:resource="&fibo-sec-fund-civ;OrganizationStrategy"/>
		<rdfs:range rdf:resource="&xsd;string"/>
		<skos:definition xml:lang="en">Other restrictions or treatment information in respect of this strategy and the organization to which it refers.</skos:definition>
	</owl:DatatypeProperty>
	
	<owl:ObjectProperty rdf:about="&fibo-sec-fund-civ;administeredBy">
		<rdfs:subPropertyOf rdf:resource="&fibo-sec-fund-civ;fundHasRelatedParty"/>
		<rdfs:label xml:lang="en">administered by</rdfs:label>
		<rdfs:domain rdf:resource="&fibo-sec-sec-pls;CollectiveInvestmentVehicle"/>
		<rdfs:range rdf:resource="&fibo-sec-fund-civ;FundAdministrator"/>
	</owl:ObjectProperty>
	
	<owl:ObjectProperty rdf:about="&fibo-sec-fund-civ;advisedBy">
		<rdfs:subPropertyOf rdf:resource="&fibo-sec-fund-civ;fundHasRelatedParty"/>
		<rdfs:label xml:lang="en">advised by</rdfs:label>
		<rdfs:domain rdf:resource="&fibo-sec-sec-pls;CollectiveInvestmentVehicle"/>
		<rdfs:range rdf:resource="&fibo-sec-fund-civ;InvestmentAdvisor"/>
	</owl:ObjectProperty>
	
	<owl:ObjectProperty rdf:about="&fibo-sec-fund-civ;anticipatedVolatility">
		<rdfs:label xml:lang="en">anticipated volatility</rdfs:label>
		<rdfs:domain rdf:resource="&fibo-sec-fund-civ;FundProspectus"/>
		<rdfs:range rdf:resource="&cmns-qtu;Percentage"/>
	</owl:ObjectProperty>
	
	<owl:ObjectProperty rdf:about="&fibo-sec-fund-civ;anticipates">
		<rdfs:label xml:lang="en">anticipates</rdfs:label>
		<rdfs:domain rdf:resource="&fibo-sec-fund-civ;FundProspectus"/>
		<rdfs:range rdf:resource="&fibo-ind-ind-ind;MarketRate"/>
	</owl:ObjectProperty>
	
	<owl:ObjectProperty rdf:about="&fibo-sec-fund-civ;assessedAgainst">
		<rdfs:label xml:lang="en">assessed against</rdfs:label>
		<rdfs:domain rdf:resource="&fibo-sec-fund-civ;FundPortfolio"/>
		<rdfs:range rdf:resource="&fibo-sec-fund-civ;PortfolioBenchmark"/>
	</owl:ObjectProperty>
	
	<owl:ObjectProperty rdf:about="&fibo-sec-fund-civ;authorizedCountry">
		<rdfs:label xml:lang="en">authorized country</rdfs:label>
		<rdfs:domain rdf:resource="&fibo-sec-fund-civ;FundProcessingGeneralTerms"/>
		<rdfs:range rdf:resource="&cmns-loc;Country"/>
		<skos:definition xml:lang="en">Country in which it is authorised to commercialise the fund.</skos:definition>
	</owl:ObjectProperty>
	
	<owl:DatatypeProperty rdf:about="&fibo-sec-fund-civ;backEndLoadApplicable">
		<rdfs:label xml:lang="en">back end load applicable</rdfs:label>
		<rdfs:domain rdf:resource="&fibo-sec-fund-civ;FundProcessingGeneralTerms"/>
		<rdfs:range rdf:resource="&xsd;boolean"/>
		<skos:definition xml:lang="en">Whether an exit charge, eg, CDSC, on redemption orders for this class can be applied.</skos:definition>
	</owl:DatatypeProperty>
	
	<owl:ObjectProperty rdf:about="&fibo-sec-fund-civ;benchmarkWeight">
		<rdfs:label xml:lang="en">benchmark weight</rdfs:label>
		<rdfs:domain rdf:resource="&fibo-sec-fund-civ;PortfolioBenchmark"/>
		<rdfs:range rdf:resource="&cmns-qtu;Percentage"/>
		<skos:definition xml:lang="en">Instrument weighting in the benchmark for the portfolio.</skos:definition>
	</owl:ObjectProperty>
	
	<owl:DatatypeProperty rdf:about="&fibo-sec-fund-civ;blacklisted">
		<rdfs:label xml:lang="en">blacklisted</rdfs:label>
		<rdfs:domain rdf:resource="&fibo-sec-fund-civ;OrganizationStrategy"/>
		<rdfs:range rdf:resource="&xsd;boolean"/>
		<skos:definition xml:lang="en">Whether or not the strategy in framed so as to include the referenced business entity as being blacklisted. If yes, the strategy prevents investment in securities issued by that organization.</skos:definition>
	</owl:DatatypeProperty>
	
	<owl:DatatypeProperty rdf:about="&fibo-sec-fund-civ;clearFundsRequired">
		<rdfs:label xml:lang="en">clear funds required</rdfs:label>
		<rdfs:domain rdf:resource="&fibo-fbc-pas-fpas;SettlementTerms"/>
		<rdfs:range rdf:resource="&xsd;boolean"/>
		<skos:definition xml:lang="en">Whether cleared funds may be required before a subscription order can be executed.</skos:definition>
	</owl:DatatypeProperty>
	
	<owl:ObjectProperty rdf:about="&fibo-sec-fund-civ;couponPaymentDate">
		<rdfs:label xml:lang="en">coupon payment date</rdfs:label>
		<rdfs:domain rdf:resource="&fibo-sec-fund-civ;FundCouponPolicy"/>
		<rdfs:range rdf:resource="&fibo-fnd-dt-bd;DayOfMonth"/>
		<skos:definition xml:lang="en">The date at which the coupon is distributed to the bond unit holder.</skos:definition>
	</owl:ObjectProperty>
	
	<owl:DatatypeProperty rdf:about="&fibo-sec-fund-civ;dealingFrequencyDescription">
		<rdfs:label xml:lang="en">dealing frequency description</rdfs:label>
		<rdfs:domain rdf:resource="&fibo-sec-fund-civ;FundProcessingTerms"/>
		<rdfs:range rdf:resource="&xsd;string"/>
		<skos:definition xml:lang="en">Description of frequency at which the subscriptions and redemptions are done.</skos:definition>
	</owl:DatatypeProperty>
	
	<owl:DatatypeProperty rdf:about="&fibo-sec-fund-civ;declarationChannel">
		<rdfs:label xml:lang="en">declaration channel</rdfs:label>
		<rdfs:domain rdf:resource="&fibo-sec-fund-civ;NetAssetValueCalculationMethod"/>
		<rdfs:range rdf:resource="&xsd;string"/>
		<skos:definition xml:lang="en">Means of the net asset value publication, eg, a newspaper.</skos:definition>
	</owl:DatatypeProperty>
	
	<owl:ObjectProperty rdf:about="&fibo-sec-fund-civ;definedInRelationTo">
		<rdfs:label xml:lang="en">defined in relation to</rdfs:label>
		<rdfs:domain rdf:resource="&fibo-sec-fund-civ;OrganizationStrategy"/>
		<rdfs:range rdf:resource="&fibo-be-le-cb;Corporation"/>
	</owl:ObjectProperty>
	
	<owl:ObjectProperty rdf:about="&fibo-sec-fund-civ;definesAllocations">
		<rdfs:subPropertyOf rdf:resource="&cmns-dsg;defines"/>
		<rdfs:label xml:lang="en">defines allocations</rdfs:label>
		<rdfs:domain rdf:resource="&fibo-sec-fund-civ;FundPortfolioInvestmentPolicy"/>
		<rdfs:range rdf:resource="&fibo-sec-fund-civ;FundPortfolioInvestmentLimitations"/>
	</owl:ObjectProperty>
	
	<owl:ObjectProperty rdf:about="&fibo-sec-fund-civ;definesBenchmark">
		<rdfs:label xml:lang="en">defines benchmark</rdfs:label>
		<rdfs:domain rdf:resource="&fibo-sec-fund-civ;PortfolioBenchmark"/>
		<rdfs:range rdf:resource="&fibo-ind-ind-ind;MarketRate"/>
	</owl:ObjectProperty>
	
	<owl:ObjectProperty rdf:about="&fibo-sec-fund-civ;definesMainFundOrderDeskAccount">
		<rdfs:label xml:lang="en">defines main fund order desk account</rdfs:label>
		<rdfs:domain rdf:resource="&fibo-sec-fund-civ;FundProcessingTerms"/>
		<rdfs:range rdf:resource="&fibo-sec-fund-civ;FundsProcessingAccount"/>
	</owl:ObjectProperty>
	
	<owl:ObjectProperty rdf:about="&fibo-sec-fund-civ;distributedBy">
		<rdfs:subPropertyOf rdf:resource="&fibo-sec-fund-civ;fundHasRelatedParty"/>
		<rdfs:label xml:lang="en">distributed by</rdfs:label>
		<rdfs:domain rdf:resource="&fibo-sec-sec-pls;CollectiveInvestmentVehicle"/>
		<rdfs:range rdf:resource="&fibo-sec-fund-civ;FundDistributor"/>
	</owl:ObjectProperty>
	
	<owl:DatatypeProperty rdf:about="&fibo-sec-fund-civ;distributionWithReinvestment">
		<rdfs:label xml:lang="en">distribution with reinvestment</rdfs:label>
		<rdfs:domain rdf:resource="&fibo-sec-fund-civ;FundReinvestmentPolicy"/>
		<rdfs:domain rdf:resource="&fibo-sec-fund-civ;FundUnitDistributionPolicy"/>
		<rdfs:range rdf:resource="&xsd;boolean"/>
		<skos:definition xml:lang="en">It is possible to hold shares for which the accrued income is distributed, but then reinvested automatically in additional units/shares allocated to the investor.</skos:definition>
	</owl:DatatypeProperty>
	
	<owl:DatatypeProperty rdf:about="&fibo-sec-fund-civ;dualFund">
		<rdfs:label xml:lang="en">dual fund</rdfs:label>
		<rdfs:domain rdf:resource="&fibo-sec-fund-civ;FundProcessingGeneralTerms"/>
		<rdfs:range rdf:resource="&xsd;boolean"/>
		<skos:definition xml:lang="en">Whether the fund has two prices.</skos:definition>
	</owl:DatatypeProperty>
	
	<owl:ObjectProperty rdf:about="&fibo-sec-fund-civ;endOfFiscalYear">
		<rdfs:label xml:lang="en">end of fiscal year</rdfs:label>
		<rdfs:range rdf:resource="&fibo-fnd-dt-bd;DayOfMonth"/>
		<skos:definition xml:lang="en">Day and month on any given year at which the books are closed and profit and loss is determined.</skos:definition>
	</owl:ObjectProperty>
	
	<owl:ObjectProperty rdf:about="&fibo-sec-fund-civ;exCouponDate">
		<rdfs:label xml:lang="en">ex coupon date</rdfs:label>
		<rdfs:domain rdf:resource="&fibo-sec-fund-civ;FundCouponPolicy"/>
		<rdfs:range rdf:resource="&fibo-fnd-dt-bd;DayOfMonth"/>
		<skos:definition xml:lang="en">The date at which the coupon is substracted from the NAV</skos:definition>
	</owl:ObjectProperty>
	
	<owl:DatatypeProperty rdf:about="&fibo-sec-fund-civ;firstAccountingYearEndDate">
		<rdfs:label xml:lang="en">first accounting year end date</rdfs:label>
		<skos:definition xml:lang="en">Last day of the first accounting year for the fund.</skos:definition>
	</owl:DatatypeProperty>
	
	<owl:DatatypeProperty rdf:about="&fibo-sec-fund-civ;firstNAVCalculationDate">
		<rdfs:label xml:lang="en">first n a v calculation date</rdfs:label>
		<rdfs:domain rdf:resource="&fibo-sec-sec-pls;CollectiveInvestmentVehicle"/>
		<skos:definition xml:lang="en">The first date of NAV calculation</skos:definition>
	</owl:DatatypeProperty>
	
	<owl:DatatypeProperty rdf:about="&fibo-sec-fund-civ;frontEndLoadApplicable">
		<rdfs:label xml:lang="en">front end load applicable</rdfs:label>
		<rdfs:domain rdf:resource="&fibo-sec-fund-civ;FundSubscriptionTerms"/>
		<rdfs:range rdf:resource="&xsd;boolean"/>
		<skos:definition xml:lang="en">Whether a front end charge on subscription orders for this class can be applied.</skos:definition>
	</owl:DatatypeProperty>
	
	<owl:DatatypeProperty rdf:about="&fibo-sec-fund-civ;fundClassTypeIdentifier">
		<rdfs:label xml:lang="en">fund class type identifier</rdfs:label>
		<rdfs:domain rdf:resource="&fibo-sec-fund-fund;FundUnit"/>
		<rdfs:range rdf:resource="&xsd;string"/>
		<skos:definition xml:lang="en">A textual identification of the class of fund units. This is used to uniquely identify a particular class of fund units, and thereby identify features of this type of unit within the fund.</skos:definition>
	</owl:DatatypeProperty>
	
	<owl:ObjectProperty rdf:about="&fibo-sec-fund-civ;fundHasRelatedParty">
		<rdfs:label xml:lang="en">fund has related party</rdfs:label>
		<rdfs:domain rdf:resource="&fibo-sec-sec-pls;CollectiveInvestmentVehicle"/>
		<rdfs:range rdf:resource="&fibo-sec-fund-civ;FundsProcessingParty"/>
	</owl:ObjectProperty>
	
	<owl:ObjectProperty rdf:about="&fibo-sec-fund-civ;givesOwnershipOf">
		<rdfs:label xml:lang="en">gives ownership of</rdfs:label>
		<rdfs:domain rdf:resource="&fibo-sec-fund-civ;StakeInFund"/>
		<rdfs:range rdf:resource="&fibo-sec-sec-pls;CollectiveInvestmentVehicle"/>
	</owl:ObjectProperty>
	
	<owl:ObjectProperty rdf:about="&fibo-sec-fund-civ;hasAdditionalInformation">
		<rdfs:label xml:lang="en">has additional information</rdfs:label>
		<rdfs:domain rdf:resource="&fibo-sec-sec-pls;CollectiveInvestmentVehicle"/>
		<rdfs:range rdf:resource="&fibo-sec-fund-civ;OtherInvestmentFundInformation"/>
	</owl:ObjectProperty>
	
	<owl:ObjectProperty rdf:about="&fibo-sec-fund-civ;hasAdditionalRedemptionRestrictions">
		<rdfs:label xml:lang="en">has additional redemption restrictions</rdfs:label>
		<rdfs:domain rdf:resource="&fibo-sec-fund-civ;FundRedemptionTerms"/>
		<rdfs:range rdf:resource="&fibo-sec-fund-civ;ReferToFundOrderDesk"/>
	</owl:ObjectProperty>
	
	<owl:ObjectProperty rdf:about="&fibo-sec-fund-civ;hasAuditor">
		<rdfs:subPropertyOf rdf:resource="&fibo-sec-fund-civ;fundHasRelatedParty"/>
		<rdfs:label xml:lang="en">has auditor</rdfs:label>
		<rdfs:domain rdf:resource="&fibo-sec-sec-pls;CollectiveInvestmentVehicle"/>
		<rdfs:range rdf:resource="&fibo-sec-fund-civ;FundAuditor"/>
	</owl:ObjectProperty>
	
	<owl:ObjectProperty rdf:about="&fibo-sec-fund-civ;hasContactDetails">
		<rdfs:label xml:lang="en">has contact details</rdfs:label>
		<rdfs:domain rdf:resource="&fibo-sec-fund-civ;PortfolioManager"/>
	</owl:ObjectProperty>
	
	<owl:ObjectProperty rdf:about="&fibo-sec-fund-civ;hasDataProvider">
		<rdfs:subPropertyOf rdf:resource="&fibo-sec-fund-civ;fundHasRelatedParty"/>
		<rdfs:label xml:lang="en">has data provider</rdfs:label>
		<rdfs:domain rdf:resource="&fibo-sec-sec-pls;CollectiveInvestmentVehicle"/>
		<rdfs:range rdf:resource="&fibo-be-fct-pub;MarketDataProvider"/>
		<skos:definition xml:lang="en">has an organization which is the data provider and is legally responsible for the information provided</skos:definition>
	</owl:ObjectProperty>
	
	<owl:ObjectProperty rdf:about="&fibo-sec-fund-civ;hasDefaultSettlementConvention">
		<rdfs:label xml:lang="en">has default settlement convention</rdfs:label>
		<rdfs:domain rdf:resource="&fibo-sec-fund-civ;FundProcessingTerms"/>
		<rdfs:range rdf:resource="&fibo-fbc-fi-stl;SettlementConvention"/>
	</owl:ObjectProperty>
	
	<owl:ObjectProperty rdf:about="&fibo-sec-fund-civ;hasDepository">
		<rdfs:subPropertyOf rdf:resource="&fibo-sec-fund-civ;fundHasRelatedParty"/>
		<rdfs:label xml:lang="en">has depository</rdfs:label>
		<rdfs:domain rdf:resource="&fibo-sec-sec-pls;CollectiveInvestmentVehicle"/>
		<rdfs:range rdf:resource="&fibo-sec-fund-civ;FundDepositary"/>
	</owl:ObjectProperty>
	
	<owl:ObjectProperty rdf:about="&fibo-sec-fund-civ;hasDetails">
		<rdfs:label xml:lang="en">has details</rdfs:label>
		<rdfs:domain rdf:resource="&fibo-sec-fund-fund;FundUnit"/>
		<rdfs:range rdf:resource="&fibo-sec-fund-civ;NetAssetValueCalculationMethod"/>
		<skos:definition xml:lang="en">Information on the net asset value calculation of the investment fund component.</skos:definition>
	</owl:ObjectProperty>
	
	<owl:ObjectProperty rdf:about="&fibo-sec-fund-civ;hasExpectedCoupon">
		<rdfs:label xml:lang="en">has expected coupon</rdfs:label>
		<rdfs:domain rdf:resource="&fibo-sec-fund-civ;FundBondClassUnit"/>
		<rdfs:range rdf:resource="&fibo-sec-fund-civ;FundBondUnitCoupon"/>
	</owl:ObjectProperty>
	
	<owl:ObjectProperty rdf:about="&fibo-sec-fund-civ;hasFundPolicy">
		<rdfs:label xml:lang="en">has fund policy</rdfs:label>
		<rdfs:domain rdf:resource="&fibo-sec-sec-pls;CollectiveInvestmentVehicle"/>
		<rdfs:range rdf:resource="&fibo-sec-fund-civ;FundInvestmentPolicy"/>
		<skos:definition xml:lang="en">Overall policy for amounts invested, limitations etc. Not the same as the detailed Portfolio policy.</skos:definition>
	</owl:ObjectProperty>
	
	<owl:ObjectProperty rdf:about="&fibo-sec-fund-civ;hasFundProcessingTerms">
		<rdfs:subPropertyOf rdf:resource="&fibo-fnd-agr-ctr;hasContractualElement"/>
		<rdfs:label xml:lang="en">has fund processing terms</rdfs:label>
		<rdfs:domain rdf:resource="&fibo-sec-fund-fund;FundUnit"/>
		<rdfs:range rdf:resource="&fibo-sec-fund-civ;FundProcessingTerms"/>
	</owl:ObjectProperty>
	
	<owl:ObjectProperty rdf:about="&fibo-sec-fund-civ;hasIntendedRiskLevel">
		<rdfs:label xml:lang="en">has intended risk level</rdfs:label>
		<rdfs:domain rdf:resource="&fibo-sec-fund-civ;FundInvestmentObjective"/>
		<rdfs:range rdf:resource="&fibo-sec-fund-civ;RiskLevel"/>
	</owl:ObjectProperty>
	
	<owl:ObjectProperty rdf:about="&fibo-sec-fund-civ;hasInvestmentStrategy">
		<rdfs:label xml:lang="en">strategy</rdfs:label>
		<rdfs:domain rdf:resource="&fibo-sec-sec-ast;Portfolio"/>
		<rdfs:range rdf:resource="&fibo-sec-fund-civ;InvestmentStrategy"/>
	</owl:ObjectProperty>
	
	<owl:ObjectProperty rdf:about="&fibo-sec-fund-civ;hasIssueDate">
		<rdfs:label xml:lang="en">has issue date</rdfs:label>
		<rdfs:domain rdf:resource="&fibo-sec-fund-fund;FundUnit"/>
		<rdfs:range rdf:resource="&cmns-dt;Date"/>
		<skos:definition xml:lang="en">Date of first NAV calculation and start of performance calculations (same as launch date)</skos:definition>
	</owl:ObjectProperty>
	
	<owl:ObjectProperty rdf:about="&fibo-sec-fund-civ;hasLiquidity">
		<rdfs:label xml:lang="en">has liquidity</rdfs:label>
		<rdfs:domain rdf:resource="&fibo-sec-fund-civ;FundPortfolio"/>
		<rdfs:range rdf:resource="&fibo-sec-fund-civ;Liquidity"/>
	</owl:ObjectProperty>
	
	<owl:ObjectProperty rdf:about="&fibo-sec-fund-civ;hasManagementCompany">
		<rdfs:subPropertyOf rdf:resource="&fibo-sec-fund-civ;fundHasRelatedParty"/>
		<rdfs:label xml:lang="en">has management company</rdfs:label>
		<rdfs:domain rdf:resource="&fibo-sec-sec-pls;CollectiveInvestmentVehicle"/>
		<rdfs:range rdf:resource="&fibo-sec-fund-civ;FundManager"/>
	</owl:ObjectProperty>
	
	<owl:ObjectProperty rdf:about="&fibo-sec-fund-civ;hasPolicyTerms">
		<rdfs:label xml:lang="en">has policy terms</rdfs:label>
		<rdfs:domain rdf:resource="&fibo-sec-fund-civ;FundBondUnitCoupon"/>
		<rdfs:range rdf:resource="&fibo-sec-fund-civ;FundCouponPolicy"/>
	</owl:ObjectProperty>
	
	<owl:ObjectProperty rdf:about="&fibo-sec-fund-civ;hasPortfolio">
		<rdfs:label xml:lang="en">has portfolio</rdfs:label>
		<rdfs:domain rdf:resource="&fibo-sec-sec-pls;CollectiveInvestmentVehicle"/>
		<rdfs:range rdf:resource="&fibo-sec-fund-civ;FundPortfolio"/>
	</owl:ObjectProperty>
	
	<owl:ObjectProperty rdf:about="&fibo-sec-fund-civ;hasRelatedFundTerms">
		<rdfs:subPropertyOf rdf:resource="&fibo-sec-fund-civ;hasRelatedTerms"/>
		<rdfs:label xml:lang="en">has related fund terms</rdfs:label>
		<rdfs:domain rdf:resource="&fibo-sec-sec-pls;CollectiveInvestmentVehicle"/>
		<rdfs:range rdf:resource="&fibo-sec-fund-civ;FundProcessingTerms"/>
	</owl:ObjectProperty>
	
	<owl:ObjectProperty rdf:about="&fibo-sec-fund-civ;hasRelatedTerms">
		<rdfs:label xml:lang="en">has related terms</rdfs:label>
		<rdfs:range rdf:resource="&fibo-fnd-agr-ctr;ContractualElement"/>
	</owl:ObjectProperty>
	
	<owl:ObjectProperty rdf:about="&fibo-sec-fund-civ;hasSubscriptionTerms">
		<rdfs:subPropertyOf rdf:resource="&fibo-sec-fund-civ;hasRelatedFundTerms"/>
		<rdfs:label xml:lang="en">has subscription terms</rdfs:label>
		<rdfs:domain rdf:resource="&fibo-sec-sec-pls;CollectiveInvestmentVehicle"/>
		<rdfs:range rdf:resource="&fibo-sec-fund-civ;FundSubscriptionTerms"/>
	</owl:ObjectProperty>
	
	<owl:ObjectProperty rdf:about="&fibo-sec-fund-civ;hasTradableUnit">
		<rdfs:label xml:lang="en">has tradable unit</rdfs:label>
		<rdfs:domain rdf:resource="&fibo-sec-sec-pls;CollectiveInvestmentVehicle"/>
		<rdfs:range rdf:resource="&fibo-sec-fund-fund;FundUnit"/>
	</owl:ObjectProperty>
	
	<owl:ObjectProperty rdf:about="&fibo-sec-fund-civ;hasTransferAgent">
		<rdfs:subPropertyOf rdf:resource="&fibo-sec-fund-civ;fundHasRelatedParty"/>
		<rdfs:label xml:lang="en">has transfer agent</rdfs:label>
		<rdfs:domain rdf:resource="&fibo-sec-sec-pls;CollectiveInvestmentVehicle"/>
		<rdfs:range rdf:resource="&fibo-sec-fund-civ;FundTransferAgent"/>
	</owl:ObjectProperty>
	
	<owl:DatatypeProperty rdf:about="&fibo-sec-fund-civ;historicPricingIndicator">
		<rdfs:label xml:lang="en">historic pricing indicator</rdfs:label>
		<rdfs:domain rdf:resource="&fibo-sec-fund-civ;NetAssetValueCalculationMethod"/>
		<rdfs:range rdf:resource="&xsd;boolean"/>
		<skos:definition xml:lang="en">Indicates whether the price is historic or forward.</skos:definition>
	</owl:DatatypeProperty>
	
	<owl:DatatypeProperty rdf:about="&fibo-sec-fund-civ;holderMayReinvest">
		<rdfs:label xml:lang="en">holder may reinvest</rdfs:label>
		<rdfs:domain rdf:resource="&fibo-sec-fund-civ;DistributingShareClass"/>
		<rdfs:range rdf:resource="&xsd;boolean"/>
		<skos:definition xml:lang="en">Whether or not the holder may reinvest dividends in the fund.</skos:definition>
	</owl:DatatypeProperty>
	
	<owl:DatatypeProperty rdf:about="&fibo-sec-fund-civ;holdingTransferable">
		<rdfs:label xml:lang="en">holding transferable</rdfs:label>
		<rdfs:domain rdf:resource="&fibo-sec-fund-civ;FundProcessingGeneralTerms"/>
		<rdfs:range rdf:resource="&xsd;boolean"/>
		<skos:definition xml:lang="en">Whether registered investors are able to transfer some or all of their holdings to third parties.</skos:definition>
	</owl:DatatypeProperty>
	
	<owl:ObjectProperty rdf:about="&fibo-sec-fund-civ;identifiesAssetTypesBy">
		<rdfs:label xml:lang="en">identifies asset types by</rdfs:label>
		<rdfs:domain rdf:resource="&fibo-sec-fund-civ;AssetClassStrategy"/>
		<rdfs:range rdf:resource="&fibo-sec-sec-cls;FinancialInstrumentClassifier"/>
	</owl:ObjectProperty>
	
	<owl:ObjectProperty rdf:about="&fibo-sec-fund-civ;implementsFundPolicy">
		<rdfs:label xml:lang="en">implements fund policy</rdfs:label>
		<rdfs:domain rdf:resource="&fibo-sec-fund-civ;FundPortfolio"/>
		<rdfs:range rdf:resource="&fibo-sec-fund-civ;FundPortfolioInvestmentPolicy"/>
	</owl:ObjectProperty>
	
	<owl:ObjectProperty rdf:about="&fibo-sec-fund-civ;inceptionDate">
		<rdfs:label xml:lang="en">inception date</rdfs:label>
		<rdfs:domain rdf:resource="&fibo-sec-sec-pls;CollectiveInvestmentVehicle"/>
		<rdfs:range rdf:resource="&cmns-dt;Date"/>
		<skos:definition xml:lang="en">Authorization date in the country of origin.</skos:definition>
	</owl:ObjectProperty>
	
	<owl:ObjectProperty rdf:about="&fibo-sec-fund-civ;inceptionDate.1">
		<rdfs:label xml:lang="en">inception date</rdfs:label>
		<rdfs:domain rdf:resource="&fibo-sec-fund-civ;FundShareClassUnit"/>
		<rdfs:range rdf:resource="&cmns-dt;Date"/>
		<skos:definition xml:lang="en">Authorization date in the country of origin. Further Notes See definition in Inception Date for Fund. Separate fact exists here. Same definition used. EFAMA Review notes: Inception Date exists as soon as there is a prospectus, so it is a fact about a Share Class even if the share class is never formally issued or offered to the public. Legal structure exists even if something is not launched. Editor question: Review stated this was a fact about Share Class; confirm this fact does not apply to Bond and Note units, or was the term Share Class being used to mean all three? Meanwhile I have put the term &quot;Issue Date&quot; as a fact about all Fund Unit, as this is given a sa separate term in the EFAMA DD spreadsheet. MAy come clearer in the next version of that.</skos:definition>
	</owl:ObjectProperty>
	
	<owl:DatatypeProperty rdf:about="&fibo-sec-fund-civ;includeRelatedFirms">
		<rdfs:label xml:lang="en">include related firms</rdfs:label>
		<rdfs:domain rdf:resource="&fibo-sec-fund-civ;OrganizationStrategy"/>
		<rdfs:range rdf:resource="&xsd;boolean"/>
		<skos:definition xml:lang="en">Whether or not the strategy includes firms which are related in some way to the referenced organization.</skos:definition>
	</owl:DatatypeProperty>
	
	<owl:DatatypeProperty rdf:about="&fibo-sec-fund-civ;inclusion">
		<rdfs:label xml:lang="en">inclusion</rdfs:label>
		<rdfs:domain rdf:resource="&fibo-sec-fund-civ;FundPortfolioInvestmentLimitations"/>
		<rdfs:range rdf:resource="&xsd;boolean"/>
		<skos:definition xml:lang="en">Whether the referred strategy is included. No means this description refers to the exclusion of what is described, from the portfolio.</skos:definition>
	</owl:DatatypeProperty>
	
	<owl:ObjectProperty rdf:about="&fibo-sec-fund-civ;initialApplicationForm">
		<rdfs:label xml:lang="en">initial application form</rdfs:label>
		<rdfs:domain rdf:resource="&fibo-sec-fund-civ;FundSubscriptionTerms"/>
		<skos:definition xml:lang="en">Physical application form for the initial subscription by the investor.</skos:definition>
	</owl:ObjectProperty>
	
	<owl:DatatypeProperty rdf:about="&fibo-sec-fund-civ;investmentFocus">
		<rdfs:label xml:lang="en">investment focus</rdfs:label>
		<rdfs:domain rdf:resource="&fibo-sec-fund-civ;PortfolioInvestmentStrategy"/>
		<rdfs:range rdf:resource="&xsd;string"/>
		<skos:definition xml:lang="en">The information about the area the fund is mostly invested into (for example stock market in Germany).</skos:definition>
	</owl:DatatypeProperty>
	
	<owl:ObjectProperty rdf:about="&fibo-sec-fund-civ;isCalculatedIn">
		<rdfs:label xml:lang="en">is calculated in</rdfs:label>
		<rdfs:domain rdf:resource="&fibo-sec-fund-civ;NetAssetValueCalculationMethod"/>
		<rdfs:range rdf:resource="&fibo-fnd-acc-cur;Currency"/>
	</owl:ObjectProperty>
	
	<owl:ObjectProperty rdf:about="&fibo-sec-fund-civ;isUnitHolder">
		<rdfs:label xml:lang="en">is unit holder</rdfs:label>
		<rdfs:domain rdf:resource="&fibo-be-oac-opty;Investor"/>
		<rdfs:range rdf:resource="&fibo-sec-fund-fund;FundUnit"/>
	</owl:ObjectProperty>
	
	<owl:ObjectProperty rdf:about="&fibo-sec-fund-civ;issuePrice">
		<rdfs:label xml:lang="en">issue price</rdfs:label>
		<rdfs:domain rdf:resource="&fibo-sec-fund-fund;FundUnit"/>
		<rdfs:range rdf:resource="&fibo-fnd-acc-cur;Price"/>
		<skos:definition xml:lang="en">The price at which the Fund Unit was first issued.</skos:definition>
	</owl:ObjectProperty>
	
	<owl:DatatypeProperty rdf:about="&fibo-sec-fund-civ;launchDate">
		<rdfs:label xml:lang="en">launch date</rdfs:label>
		<rdfs:domain rdf:resource="&fibo-sec-sec-pls;CollectiveInvestmentVehicle"/>
		<skos:definition xml:lang="en">Date of first NAV calculation and start of performance calculations</skos:definition>
	</owl:DatatypeProperty>
	
	<owl:DatatypeProperty rdf:about="&fibo-sec-fund-civ;limitedSharesAreIssued">
		<rdfs:label xml:lang="en">limited shares are issued</rdfs:label>
		<rdfs:domain rdf:resource="&fibo-sec-fund-civ;FundShareClassUnit"/>
		<rdfs:range rdf:resource="&xsd;boolean"/>
		<skos:definition xml:lang="en">Whether or not new shares can be issued in the fund. This is what makes it a closed end or open end fund.</skos:definition>
	</owl:DatatypeProperty>
	
	<owl:DatatypeProperty rdf:about="&fibo-sec-fund-civ;mainFundOrderDesk">
		<rdfs:label xml:lang="en">main fund order desk</rdfs:label>
		<rdfs:domain rdf:resource="&fibo-sec-fund-civ;FundProcessingTerms"/>
		<rdfs:range rdf:resource="&xsd;boolean"/>
		<skos:definition xml:lang="en">Whether the fund order desk is the principal entity appointed by the fund to which orders should be submitted.</skos:definition>
	</owl:DatatypeProperty>
	
	<owl:ObjectProperty rdf:about="&fibo-sec-fund-civ;maximumDeviation">
		<rdfs:label xml:lang="en">maximum deviation</rdfs:label>
		<rdfs:domain rdf:resource="&fibo-sec-fund-civ;PortfolioBenchmark"/>
		<rdfs:range rdf:resource="&cmns-qtu;Percentage"/>
		<skos:definition xml:lang="en">Maximum allowable deviation from the benchmark.</skos:definition>
	</owl:ObjectProperty>
	
	<owl:ObjectProperty rdf:about="&fibo-sec-fund-civ;maximumInvestmentAmount">
		<rdfs:label xml:lang="en">maximum investment amount</rdfs:label>
		<rdfs:domain rdf:resource="&fibo-sec-fund-civ;FundPortfolioInvestmentLimitations"/>
		<rdfs:range rdf:resource="&fibo-fnd-acc-cur;MonetaryAmount"/>
		<skos:definition xml:lang="en">Maximum amount that may be invested in the specified strategy.</skos:definition>
	</owl:ObjectProperty>
	
	<owl:ObjectProperty rdf:about="&fibo-sec-fund-civ;maximumInvestmentPercentage">
		<rdfs:label xml:lang="en">maximum investment percentage</rdfs:label>
		<rdfs:domain rdf:resource="&fibo-sec-fund-civ;FundPortfolioInvestmentLimitations"/>
		<rdfs:range rdf:resource="&cmns-qtu;Percentage"/>
		<skos:definition xml:lang="en">Maximum percentage that may be invested in the specified strategy.</skos:definition>
	</owl:ObjectProperty>
	
	<owl:ObjectProperty rdf:about="&fibo-sec-fund-civ;maximumPurchasingFee">
		<rdfs:label xml:lang="en">maximum purchasing fee</rdfs:label>
		<rdfs:domain rdf:resource="&fibo-sec-fund-civ;FundSubscriptionTerms"/>
		<rdfs:range rdf:resource="&fibo-fbc-pas-caa;Fee"/>
		<skos:definition xml:lang="en">Maximum percentage or fixed amount of money due when purchasing fund shares Definition origin:EFAMA DD</skos:definition>
	</owl:ObjectProperty>
	
	<owl:ObjectProperty rdf:about="&fibo-sec-fund-civ;maximumRedemptionAmount">
		<rdfs:label xml:lang="en">maximum redemption amount</rdfs:label>
		<rdfs:domain rdf:resource="&fibo-sec-fund-civ;FundRedemptionTerms"/>
		<rdfs:range rdf:resource="&fibo-fnd-acc-cur;MonetaryAmount"/>
		<skos:definition xml:lang="en">Maximum quantity of securities, expressed as an amount that can be sold.</skos:definition>
	</owl:ObjectProperty>
	
	<owl:ObjectProperty rdf:about="&fibo-sec-fund-civ;maximumRedemptionFee">
		<rdfs:label xml:lang="en">maximum redemption fee</rdfs:label>
		<rdfs:domain rdf:resource="&fibo-sec-fund-civ;FundSubscriptionTerms"/>
		<rdfs:range rdf:resource="&fibo-fbc-pas-caa;Fee"/>
		<skos:definition xml:lang="en">Maximum percentage or fixed amount of money due when redeeming fund shares Definition origin:EFAMA DD</skos:definition>
	</owl:ObjectProperty>
	
	<owl:ObjectProperty rdf:about="&fibo-sec-fund-civ;maximumRedemptionPercentage">
		<rdfs:label xml:lang="en">maximum redemption percentage</rdfs:label>
		<rdfs:domain rdf:resource="&fibo-sec-fund-civ;FundRedemptionTerms"/>
		<rdfs:range rdf:resource="&cmns-qtu;Percentage"/>
		<skos:definition xml:lang="en">Maximum quantity of securities, expressed as a percentage that can be sold.</skos:definition>
	</owl:ObjectProperty>
	
	<owl:DatatypeProperty rdf:about="&fibo-sec-fund-civ;maximumRedemptionUnits">
		<rdfs:label xml:lang="en">maximum redemption units</rdfs:label>
		<rdfs:domain rdf:resource="&fibo-sec-fund-civ;FundRedemptionTerms"/>
		<rdfs:range rdf:resource="&xsd;integer"/>
		<skos:definition xml:lang="en">Maximum number of shares/units that may be redeemed on a single dealing day.</skos:definition>
	</owl:DatatypeProperty>
	
	<owl:ObjectProperty rdf:about="&fibo-sec-fund-civ;mayAlsoBe">
		<rdfs:label xml:lang="en">may also be</rdfs:label>
		<rdfs:domain rdf:resource="&fibo-sec-fund-civ;FundAdministrator"/>
		<rdfs:range rdf:resource="&fibo-sec-fund-civ;UnitIssuer"/>
		<skos:definition xml:lang="en">The unit issuer would be the fund administrator (except when it is a Bond).</skos:definition>
	</owl:ObjectProperty>
	
	<owl:ObjectProperty rdf:about="&fibo-sec-fund-civ;minimumDeviation">
		<rdfs:label xml:lang="en">minimum deviation</rdfs:label>
		<rdfs:domain rdf:resource="&fibo-sec-fund-civ;PortfolioBenchmark"/>
		<rdfs:range rdf:resource="&cmns-qtu;Percentage"/>
		<skos:definition xml:lang="en">Minimum allowable deviation from the benchmark.</skos:definition>
	</owl:ObjectProperty>
	
	<owl:ObjectProperty rdf:about="&fibo-sec-fund-civ;minimumHoldingPeriod">
		<rdfs:label xml:lang="en">minimum holding period</rdfs:label>
		<rdfs:domain rdf:resource="&fibo-sec-fund-civ;FundProcessingGeneralTerms"/>
		<rdfs:range rdf:resource="&cmns-dt;Duration"/>
		<skos:definition xml:lang="en">Period, in days, during which the units/shares must be held following their issue before redemption will be permitted.</skos:definition>
	</owl:ObjectProperty>
	
	<owl:ObjectProperty rdf:about="&fibo-sec-fund-civ;minimumInitialSubscriptionAmount">
		<rdfs:label xml:lang="en">minimum initial subscription amount</rdfs:label>
		<rdfs:domain rdf:resource="&fibo-sec-fund-civ;FundSubscriptionTerms"/>
		<rdfs:range rdf:resource="&fibo-fnd-acc-cur;MonetaryAmount"/>
		<skos:definition xml:lang="en">Minimum initial subscription value.</skos:definition>
	</owl:ObjectProperty>
	
	<owl:DatatypeProperty rdf:about="&fibo-sec-fund-civ;minimumInitialSubscriptionUnits">
		<rdfs:label xml:lang="en">minimum initial subscription units</rdfs:label>
		<rdfs:domain rdf:resource="&fibo-sec-fund-civ;FundSubscriptionTerms"/>
		<rdfs:range rdf:resource="&xsd;integer"/>
		<skos:definition xml:lang="en">Minimum initial number of units/shares that must be purchased.</skos:definition>
	</owl:DatatypeProperty>
	
	<owl:ObjectProperty rdf:about="&fibo-sec-fund-civ;minimumInvestmentAmount">
		<rdfs:label xml:lang="en">minimum investment amount</rdfs:label>
		<rdfs:domain rdf:resource="&fibo-sec-fund-civ;FundPortfolioInvestmentLimitations"/>
		<rdfs:range rdf:resource="&fibo-fnd-acc-cur;MonetaryAmount"/>
		<skos:definition xml:lang="en">Minimum amount that has to be invested in the specified strategy.</skos:definition>
	</owl:ObjectProperty>
	
	<owl:ObjectProperty rdf:about="&fibo-sec-fund-civ;minimumInvestmentPercentage">
		<rdfs:label xml:lang="en">minimum investment percentage</rdfs:label>
		<rdfs:domain rdf:resource="&fibo-sec-fund-civ;FundPortfolioInvestmentLimitations"/>
		<rdfs:range rdf:resource="&cmns-qtu;Percentage"/>
		<skos:definition xml:lang="en">Minimum percentage that has to be invested in the specified strategy.</skos:definition>
	</owl:ObjectProperty>
	
	<owl:ObjectProperty rdf:about="&fibo-sec-fund-civ;minimumRatingRestriction">
		<rdfs:label xml:lang="en">minimum rating restriction</rdfs:label>
		<rdfs:domain rdf:resource="&fibo-sec-fund-civ;InvestmentRestriction"/>
		<rdfs:range rdf:resource="&fibo-fnd-arr-rt;RatingScore"/>
		<skos:definition xml:lang="en">The minimum rating of securities to be invested in.</skos:definition>
	</owl:ObjectProperty>
	
	<owl:ObjectProperty rdf:about="&fibo-sec-fund-civ;minimumRemainingHoldingAmount">
		<rdfs:label xml:lang="en">minimum remaining holding amount</rdfs:label>
		<rdfs:domain rdf:resource="&fibo-sec-fund-civ;FundProcessingGeneralTerms"/>
		<rdfs:range rdf:resource="&fibo-fnd-acc-cur;MonetaryAmount"/>
		<skos:definition xml:lang="en">Minimum value of units/shares that must be retained to avoid automatic redemption.</skos:definition>
	</owl:ObjectProperty>
	
	<owl:DatatypeProperty rdf:about="&fibo-sec-fund-civ;minimumRemainingHoldingUnits">
		<rdfs:label xml:lang="en">minimum remaining holding units</rdfs:label>
		<rdfs:domain rdf:resource="&fibo-sec-fund-civ;FundProcessingGeneralTerms"/>
		<rdfs:range rdf:resource="&xsd;integer"/>
		<skos:definition xml:lang="en">Minimum number of units/shares that must be retained to avoid automatic redemption.</skos:definition>
	</owl:DatatypeProperty>
	
	<owl:ObjectProperty rdf:about="&fibo-sec-fund-civ;minimumSubscriptionAmount">
		<rdfs:label xml:lang="en">minimum subscription amount</rdfs:label>
		<rdfs:domain rdf:resource="&fibo-sec-fund-civ;FundSubscriptionTerms"/>
		<rdfs:range rdf:resource="&fibo-fnd-acc-cur;MonetaryAmount"/>
		<skos:definition xml:lang="en">Minimum subscription value for existing investors.</skos:definition>
	</owl:ObjectProperty>
	
	<owl:DatatypeProperty rdf:about="&fibo-sec-fund-civ;minimumSubscriptionUnits">
		<rdfs:label xml:lang="en">minimum subscription units</rdfs:label>
		<rdfs:domain rdf:resource="&fibo-sec-fund-civ;FundSubscriptionTerms"/>
		<rdfs:range rdf:resource="&xsd;integer"/>
		<skos:definition xml:lang="en">Minimum number of units/shares that must be purchased by existing investors.</skos:definition>
	</owl:DatatypeProperty>
	
	<owl:DatatypeProperty rdf:about="&fibo-sec-fund-civ;name">
		<rdfs:label xml:lang="en">name</rdfs:label>
		<rdfs:domain rdf:resource="&fibo-sec-sec-pls;CollectiveInvestmentVehicle"/>
		<rdfs:range rdf:resource="&xsd;string"/>
		<skos:definition xml:lang="en">Name of the investment fund.</skos:definition>
	</owl:DatatypeProperty>
	
	<owl:DatatypeProperty rdf:about="&fibo-sec-fund-civ;name.1">
		<rdfs:label xml:lang="en">name</rdfs:label>
		<rdfs:domain rdf:resource="&fibo-sec-fund-civ;FundPortfolioInvestmentPolicy"/>
		<rdfs:range rdf:resource="&xsd;string"/>
		<skos:definition xml:lang="en">Name given to the defined strategy.</skos:definition>
	</owl:DatatypeProperty>
	
	<owl:ObjectProperty rdf:about="&fibo-sec-fund-civ;outlines">
		<rdfs:label xml:lang="en">outlines</rdfs:label>
		<rdfs:domain rdf:resource="&fibo-sec-fund-civ;FundProspectus"/>
		<rdfs:range rdf:resource="&fibo-sec-fund-civ;FundInvestmentObjective"/>
		<owl:inverseOf rdf:resource="&fibo-sec-fund-civ;statedIn"/>
	</owl:ObjectProperty>
	
	<owl:ObjectProperty rdf:about="&fibo-sec-fund-civ;percentageInvested">
		<rdfs:label xml:lang="en">percentage invested</rdfs:label>
		<rdfs:domain rdf:resource="&fibo-sec-fund-civ;InvestmentRestriction"/>
		<rdfs:range rdf:resource="&cmns-qtu;Percentage"/>
		<skos:definition xml:lang="en">The percentage of funds that is to be invested at any given time.</skos:definition>
	</owl:ObjectProperty>
	
	<owl:ObjectProperty rdf:about="&fibo-sec-fund-civ;performanceFee">
		<rdfs:label xml:lang="en">performance fee</rdfs:label>
		<rdfs:domain rdf:resource="&fibo-sec-fund-civ;FundSubscriptionTerms"/>
		<rdfs:range rdf:resource="&fibo-fbc-pas-caa;Fee"/>
		<skos:definition xml:lang="en">Fees paid for the achivements of predefined outperformance objectives Definition origin:EFAMA DD</skos:definition>
	</owl:ObjectProperty>
	
	<owl:DatatypeProperty rdf:about="&fibo-sec-fund-civ;physicalDocumentRequired">
		<rdfs:label xml:lang="en">physical document required</rdfs:label>
		<rdfs:range rdf:resource="&xsd;boolean"/>
		<skos:definition xml:lang="en">Whether a phsyical form is required through the main fund order desk. Yes: A phsyical form is required through the main fund order desk. No: A phsyical form is not required through the main fund order desk.</skos:definition>
	</owl:DatatypeProperty>
	
	<owl:ObjectProperty rdf:about="&fibo-sec-fund-civ;processingCountry">
		<rdfs:label xml:lang="en">processing country</rdfs:label>
		<rdfs:domain rdf:resource="&fibo-sec-fund-civ;FundProcessingTerms"/>
		<rdfs:range rdf:resource="&cmns-loc;Country"/>
		<skos:definition xml:lang="en">Country in which the processing characteristic applies.</skos:definition>
	</owl:ObjectProperty>
	
	<owl:DatatypeProperty rdf:about="&fibo-sec-fund-civ;productGroupDescription">
		<rdfs:label xml:lang="en">product group description</rdfs:label>
		<rdfs:domain rdf:resource="&fibo-sec-sec-pls;CollectiveInvestmentVehicle"/>
		<rdfs:range rdf:resource="&xsd;string"/>
		<skos:definition xml:lang="en">Company specific description of a group of funds.</skos:definition>
	</owl:DatatypeProperty>
	
	<owl:ObjectProperty rdf:about="&fibo-sec-fund-civ;promotedBy">
		<rdfs:subPropertyOf rdf:resource="&fibo-sec-fund-civ;fundHasRelatedParty"/>
		<rdfs:label xml:lang="en">promoted by</rdfs:label>
		<rdfs:domain rdf:resource="&fibo-sec-sec-pls;CollectiveInvestmentVehicle"/>
		<rdfs:range rdf:resource="&fibo-sec-fund-civ;FundPromoter"/>
	</owl:ObjectProperty>
	
	<owl:ObjectProperty rdf:about="&fibo-sec-fund-civ;providesDepositaryServiceFor">
		<rdfs:label xml:lang="en">provides depositary service for</rdfs:label>
		<rdfs:domain rdf:resource="&fibo-sec-fund-civ;FundDepositary"/>
		<rdfs:range rdf:resource="&fibo-sec-fund-fund;FundUnit"/>
	</owl:ObjectProperty>
	
	<owl:ObjectProperty rdf:about="&fibo-sec-fund-civ;purchasingFee">
		<rdfs:label xml:lang="en">purchasing fee</rdfs:label>
		<rdfs:domain rdf:resource="&fibo-sec-fund-civ;FundSubscriptionTerms"/>
		<rdfs:range rdf:resource="&fibo-fbc-pas-caa;Fee"/>
		<skos:definition xml:lang="en">Actual percentage or fixed amount of money due when purchasing fund shares Definition origin:EFAMA DD</skos:definition>
	</owl:ObjectProperty>
	
	<owl:ObjectProperty rdf:about="&fibo-sec-fund-civ;redemptionCutoffDateTime">
		<rdfs:label xml:lang="en">redemption cutoff date time</rdfs:label>
		<rdfs:domain rdf:resource="&fibo-sec-fund-civ;FundRedemptionTerms"/>
		<rdfs:range rdf:resource="&cmns-dt;DateTime"/>
		<skos:definition xml:lang="en">Last date/time at which an order to redeem can be given.</skos:definition>
	</owl:ObjectProperty>
	
	<owl:DatatypeProperty rdf:about="&fibo-sec-fund-civ;redemptionCycleInBusinessDays">
		<rdfs:label xml:lang="en">redemption cycle in business days</rdfs:label>
		<rdfs:domain rdf:resource="&fibo-fbc-fi-stl;SettlementConvention"/>
		<rdfs:range rdf:resource="&xsd;integer"/>
		<skos:definition xml:lang="en">The last business day following the day on which a redemption order is priced (T) by which settlement will be due for orders placed with the main Fund Order Desk. Alternatively, if proceeds will be paid following receipt of written renunciation, the last business day following receipt of the relevant renunciation documentation by the main Fund Order Desk (R) by which the proceeds will be sent.</skos:definition>
	</owl:DatatypeProperty>
	
	<owl:ObjectProperty rdf:about="&fibo-sec-fund-civ;redemptionDealingFrequency">
		<rdfs:label xml:lang="en">redemption dealing frequency</rdfs:label>
		<rdfs:domain rdf:resource="&fibo-sec-fund-civ;FundRedemptionTerms"/>
		<rdfs:range rdf:resource="&fibo-fnd-dt-fd;RecurrenceInterval"/>
		<skos:definition xml:lang="en">Frequency at which the redemptions are done.</skos:definition>
	</owl:ObjectProperty>
	
	<owl:ObjectProperty rdf:about="&fibo-sec-fund-civ;redemptionFee">
		<rdfs:label xml:lang="en">redemption fee</rdfs:label>
		<rdfs:domain rdf:resource="&fibo-sec-fund-civ;FundSubscriptionTerms"/>
		<rdfs:range rdf:resource="&fibo-fbc-pas-caa;Fee"/>
		<skos:definition xml:lang="en">Actual percentage or fixed amount of money due when redeeming fund shares Definition origin:EFAMA DD</skos:definition>
	</owl:ObjectProperty>
	
	<owl:ObjectProperty rdf:about="&fibo-sec-fund-civ;redemptionForm">
		<rdfs:label xml:lang="en">redemption form</rdfs:label>
		<rdfs:domain rdf:resource="&fibo-sec-fund-civ;FundRedemptionTerms"/>
		<skos:definition xml:lang="en">Physical written instruction/renunciation form for redemption of units/shares by the investor.</skos:definition>
	</owl:ObjectProperty>
	
	<owl:DatatypeProperty rdf:about="&fibo-sec-fund-civ;redemptionInAmountAllowed">
		<rdfs:label xml:lang="en">redemption in amount allowed</rdfs:label>
		<rdfs:domain rdf:resource="&fibo-sec-fund-civ;FundRedemptionTerms"/>
		<rdfs:range rdf:resource="&xsd;boolean"/>
		<skos:definition xml:lang="en">Whether redemptions in amount are allowed.</skos:definition>
	</owl:DatatypeProperty>
	
	<owl:ObjectProperty rdf:about="&fibo-sec-fund-civ;redemptionPeriod">
		<rdfs:label xml:lang="en">redemption period</rdfs:label>
		<rdfs:domain rdf:resource="&fibo-sec-fund-civ;FundRedemptionTerms"/>
		<rdfs:range rdf:resource="&cmns-dt;DatePeriod"/>
		<skos:definition xml:lang="en">Specific period, eg, for some guaranteed funds, during which the units/shares may be redeemed.</skos:definition>
	</owl:ObjectProperty>
	
	<owl:DatatypeProperty rdf:about="&fibo-sec-fund-civ;registrationDate">
		<rdfs:label xml:lang="en">registration date</rdfs:label>
		<rdfs:domain rdf:resource="&fibo-sec-sec-pls;CollectiveInvestmentVehicle"/>
		<skos:definition xml:lang="en">The date at which the fund is legally approved in a country other than the country of origin.</skos:definition>
	</owl:DatatypeProperty>
	
	<owl:ObjectProperty rdf:about="&fibo-sec-fund-civ;reinvestmentFrequency">
		<rdfs:label xml:lang="en">reinvestment frequency</rdfs:label>
		<rdfs:domain rdf:resource="&fibo-sec-fund-civ;FundReinvestmentPolicy"/>
		<rdfs:range rdf:resource="&fibo-fnd-dt-fd;RecurrenceInterval"/>
		<skos:definition xml:lang="en">For units where there is Reinvestment distribution, the frequency with which the reinvestment takes place (this will be the same or less frequently than the Dividend Payment Frequency), otherwise this fact does not apply.</skos:definition>
	</owl:ObjectProperty>
	
	<owl:DatatypeProperty rdf:about="&fibo-sec-fund-civ;signatureRequired">
		<rdfs:label xml:lang="en">signature required</rdfs:label>
		<rdfs:range rdf:resource="&xsd;boolean"/>
		<skos:definition xml:lang="en">Whether a phsyical form with the investor&apos;s written signature is required through the main fund order desk. Yes:A phsyical form with the investor&apos;s written signature is required through the main fund order desk.</skos:definition>
	</owl:DatatypeProperty>
	
	<owl:ObjectProperty rdf:about="&fibo-sec-fund-civ;statedDistributionFee">
		<rdfs:label xml:lang="en">stated distribution fee</rdfs:label>
		<rdfs:domain rdf:resource="&fibo-sec-fund-civ;FundProspectus"/>
		<rdfs:range rdf:resource="&fibo-fnd-acc-cur;MonetaryAmount"/>
	</owl:ObjectProperty>
	
	<owl:ObjectProperty rdf:about="&fibo-sec-fund-civ;statedIn">
		<rdfs:label xml:lang="en">stated in</rdfs:label>
		<rdfs:domain rdf:resource="&fibo-sec-fund-civ;FundInvestmentObjective"/>
		<rdfs:range rdf:resource="&fibo-sec-fund-civ;FundProspectus"/>
	</owl:ObjectProperty>
	
	<owl:DatatypeProperty rdf:about="&fibo-sec-fund-civ;statedInvestmentAim">
		<rdfs:label xml:lang="en">stated investment aim</rdfs:label>
		<rdfs:domain rdf:resource="&fibo-sec-fund-civ;FundInvestmentObjective"/>
		<rdfs:range rdf:resource="&xsd;string"/>
		<skos:definition xml:lang="en">The stated aim of the Fund in words, e.g outperfom a given benchmark.</skos:definition>
	</owl:DatatypeProperty>
	
	<owl:ObjectProperty rdf:about="&fibo-sec-fund-civ;statedManagementFee">
		<rdfs:label xml:lang="en">stated management fee</rdfs:label>
		<rdfs:domain rdf:resource="&fibo-sec-fund-civ;FundProspectus"/>
		<rdfs:range rdf:resource="&fibo-fnd-acc-cur;MonetaryAmount"/>
		<skos:definition xml:lang="en">The fee that is stated in the Prospectus as being what is to be charged for management. Further notes: Can be monetary amount or a percentage or a combination. Action: simple type is wrong.</skos:definition>
	</owl:ObjectProperty>
	
	<owl:DatatypeProperty rdf:about="&fibo-sec-fund-civ;statedObjective">
		<rdfs:label xml:lang="en">stated objective</rdfs:label>
		<rdfs:domain rdf:resource="&fibo-sec-fund-civ;FundProspectus"/>
		<rdfs:range rdf:resource="&xsd;string"/>
		<skos:definition xml:lang="en">The stated objective of the fund, in words.</skos:definition>
	</owl:DatatypeProperty>
	
	<owl:ObjectProperty rdf:about="&fibo-sec-fund-civ;stipulatesBenchmark">
		<rdfs:label xml:lang="en">stipulates benchmark</rdfs:label>
		<rdfs:domain rdf:resource="&fibo-sec-fund-civ;FundInvestmentPolicy"/>
		<rdfs:range rdf:resource="&fibo-ind-ind-ind;MarketRate"/>
	</owl:ObjectProperty>
	
	<owl:ObjectProperty rdf:about="&fibo-sec-fund-civ;subscriptionCutoffDateTime">
		<rdfs:label xml:lang="en">subscription cutoff date time</rdfs:label>
		<rdfs:domain rdf:resource="&fibo-sec-fund-civ;FundSubscriptionTerms"/>
		<rdfs:range rdf:resource="&cmns-dt;DateTime"/>
		<skos:definition xml:lang="en">Last date/time at which an order to subscribe can be given.</skos:definition>
	</owl:ObjectProperty>
	
	<owl:ObjectProperty rdf:about="&fibo-sec-fund-civ;subscriptionDealingFrequency">
		<rdfs:label xml:lang="en">subscription dealing frequency</rdfs:label>
		<rdfs:domain rdf:resource="&fibo-sec-fund-civ;FundSubscriptionTerms"/>
		<rdfs:range rdf:resource="&fibo-fnd-dt-fd;RecurrenceInterval"/>
		<skos:definition xml:lang="en">Frequency at which the subscriptions are done.</skos:definition>
	</owl:ObjectProperty>
	
	<owl:ObjectProperty rdf:about="&fibo-sec-fund-civ;subscriptionPeriod">
		<rdfs:label xml:lang="en">subscription period</rdfs:label>
		<rdfs:domain rdf:resource="&fibo-sec-fund-civ;FundSubscriptionTerms"/>
		<rdfs:range rdf:resource="&cmns-dt;DatePeriod"/>
		<skos:definition xml:lang="en">Specific period, eg, for some guaranteed funds, during which the units/shares may be subscribed to.</skos:definition>
	</owl:ObjectProperty>
	
	<owl:DatatypeProperty rdf:about="&fibo-sec-fund-civ;subscriptionsInAmountAllowed">
		<rdfs:label xml:lang="en">subscriptions in amount allowed</rdfs:label>
		<rdfs:domain rdf:resource="&fibo-sec-fund-civ;FundSubscriptionTerms"/>
		<rdfs:range rdf:resource="&xsd;boolean"/>
		<skos:definition xml:lang="en">Whether subscriptions in amount are allowed.</skos:definition>
	</owl:DatatypeProperty>
	
	<owl:ObjectProperty rdf:about="&fibo-sec-fund-civ;subsequentApplicationForm">
		<rdfs:label xml:lang="en">subsequent application form</rdfs:label>
		<rdfs:domain rdf:resource="&fibo-sec-fund-civ;FundSubscriptionTerms"/>
		<skos:definition xml:lang="en">Physical application form for subsequent investments by the same investor.</skos:definition>
	</owl:ObjectProperty>
	
	<owl:ObjectProperty rdf:about="&fibo-sec-fund-civ;supervisedBy">
		<rdfs:label xml:lang="en">supervised by</rdfs:label>
		<rdfs:domain rdf:resource="&fibo-sec-sec-pls;CollectiveInvestmentVehicle"/>
		<rdfs:range rdf:resource="&fibo-sec-fund-civ;FundSupervisoryAuthority"/>
	</owl:ObjectProperty>
	
	<owl:DatatypeProperty rdf:about="&fibo-sec-fund-civ;switchingChargeable">
		<rdfs:label xml:lang="en">switching chargeable</rdfs:label>
		<rdfs:domain rdf:resource="&fibo-sec-fund-civ;FundProcessingGeneralTerms"/>
		<rdfs:range rdf:resource="&xsd;boolean"/>
		<skos:definition xml:lang="en">Whether a switching charge for changing between sub-funds of the same umbrella can be applied.</skos:definition>
	</owl:DatatypeProperty>
	
	<owl:ObjectProperty rdf:about="&fibo-sec-fund-civ;switchingFee">
		<rdfs:label xml:lang="en">switching fee</rdfs:label>
		<rdfs:domain rdf:resource="&fibo-sec-fund-civ;FundSubscriptionTerms"/>
		<rdfs:range rdf:resource="&fibo-fbc-pas-caa;Fee"/>
		<skos:definition xml:lang="en">Actual percentage or fixed amount of money due when switching to another fund. Definition origin:EFAMA DD</skos:definition>
	</owl:ObjectProperty>
	
	<owl:ObjectProperty rdf:about="&fibo-sec-fund-civ;trackingError">
		<rdfs:label xml:lang="en">tracking error</rdfs:label>
		<rdfs:domain rdf:resource="&fibo-sec-fund-civ;InvestmentRestriction"/>
		<rdfs:range rdf:resource="&cmns-qtu;Percentage"/>
		<skos:definition xml:lang="en">See RiskFactors narrative in EFAMA DD</skos:definition>
	</owl:ObjectProperty>
	
	<owl:DatatypeProperty rdf:about="&fibo-sec-fund-civ;typeOfSecurities">
		<rdfs:label xml:lang="en">type of securities</rdfs:label>
		<rdfs:domain rdf:resource="&fibo-sec-fund-civ;InvestmentRestriction"/>
		<rdfs:range rdf:resource="&xsd;string"/>
		<skos:definition xml:lang="en">The type of securities or other holdings that may be invested in.</skos:definition>
	</owl:DatatypeProperty>
	
	<owl:ObjectProperty rdf:about="&fibo-sec-fund-civ;valuationFrequency">
		<rdfs:label xml:lang="en">valuation frequency</rdfs:label>
		<rdfs:domain rdf:resource="&fibo-sec-fund-civ;NetAssetValueCalculationMethod"/>
		<rdfs:range rdf:resource="&fibo-fnd-dt-fd;RecurrenceInterval"/>
		<skos:definition xml:lang="en">Frequency of the net asset value calculation.</skos:definition>
	</owl:ObjectProperty>
	
	<owl:DatatypeProperty rdf:about="&fibo-sec-fund-civ;valuationFrequencyTextualDescription">
		<rdfs:label xml:lang="en">valuation frequency textual description</rdfs:label>
		<rdfs:domain rdf:resource="&fibo-sec-fund-civ;NetAssetValueCalculationMethod"/>
		<rdfs:range rdf:resource="&xsd;string"/>
		<skos:definition xml:lang="en">Description of the frequency of the net asset value calculation.</skos:definition>
	</owl:DatatypeProperty>
	
	<owl:ObjectProperty rdf:about="&fibo-sec-fund-civ;valueAtRisk">
		<rdfs:label xml:lang="en">value at risk</rdfs:label>
		<rdfs:domain rdf:resource="&fibo-sec-fund-civ;InvestmentRestriction"/>
		<rdfs:range rdf:resource="&cmns-qtu;Percentage"/>
		<skos:definition xml:lang="en">See RiskClassification_NameOf in EFAMA DD Applies to Fund not Portfolio.</skos:definition>
	</owl:ObjectProperty>
	
	<owl:Class rdf:about="&fibo-sec-fund-fund;FundContract">
		<rdfs:subClassOf>
			<owl:Restriction>
				<owl:onProperty rdf:resource="&fibo-fnd-agr-ctr;isEvidencedBy"/>
				<owl:someValuesFrom rdf:resource="&fibo-sec-fund-civ;FundLegalFormDocumentation"/>
			</owl:Restriction>
		</rdfs:subClassOf>
		<cmns-av:explanatoryNote xml:lang="en">From ISO FIBIM &quot;Umbrella Fund&quot; narrative: In securities, a collective investment scheme that has a contractual or a corporate form. When it has a contractual form, a fund is constituted under either the law of contract or under the trust law and thus it is not a legal entity. In its corporate form, a fund is a legal entity and is structured as a company.</cmns-av:explanatoryNote>
	</owl:Class>
	
	<owl:Class rdf:about="&fibo-sec-fund-fund;FundUnit">
		<rdfs:subClassOf>
			<owl:Restriction>
				<owl:onProperty rdf:resource="&fibo-fnd-acc-cur;hasCurrency"/>
				<owl:someValuesFrom rdf:resource="&fibo-fnd-acc-cur;hasCurrency"/>
			</owl:Restriction>
		</rdfs:subClassOf>
		<rdfs:subClassOf>
			<owl:Restriction>
				<owl:onProperty rdf:resource="&fibo-sec-fund-civ;hasDetails"/>
				<owl:someValuesFrom rdf:resource="&fibo-sec-fund-civ;NetAssetValueCalculationMethod"/>
			</owl:Restriction>
		</rdfs:subClassOf>
		<rdfs:subClassOf>
			<owl:Restriction>
				<owl:onProperty rdf:resource="&fibo-sec-fund-civ;hasFundProcessingTerms"/>
				<owl:someValuesFrom rdf:resource="&fibo-sec-fund-civ;FundProcessingGeneralTerms"/>
			</owl:Restriction>
		</rdfs:subClassOf>
		<rdfs:subClassOf>
			<owl:Restriction>
				<owl:onProperty rdf:resource="&fibo-sec-fund-civ;hasFundProcessingTerms"/>
				<owl:someValuesFrom rdf:resource="&fibo-sec-fund-civ;FundRedemptionTerms"/>
			</owl:Restriction>
		</rdfs:subClassOf>
		<cmns-av:explanatoryNote xml:lang="en">If it is a closed fund, you can still trade the units. You trade back with the fund. Not with a counterparty. Therefore this is a tradable contract, though it may not necessarily be a transferable contract.</cmns-av:explanatoryNote>
	</owl:Class>
	
	<owl:Class rdf:about="&fibo-sec-sec-pls;CollectiveInvestmentVehicle">
		<rdfs:subClassOf>
			<owl:Restriction>
				<owl:onProperty rdf:resource="&fibo-fbc-fi-fi;isLegallyRecordedIn"/>
				<owl:someValuesFrom rdf:resource="&cmns-rga;Jurisdiction"/>
			</owl:Restriction>
		</rdfs:subClassOf>
		<rdfs:subClassOf>
			<owl:Restriction>
				<owl:onProperty rdf:resource="&fibo-fnd-acc-cur;hasCurrency"/>
				<owl:someValuesFrom rdf:resource="&fibo-fnd-acc-cur;Currency"/>
			</owl:Restriction>
		</rdfs:subClassOf>
		<rdfs:subClassOf>
			<owl:Restriction>
				<owl:onProperty rdf:resource="&fibo-fnd-gao-obj;hasStrategy"/>
				<owl:someValuesFrom rdf:resource="&fibo-sec-fund-civ;FundUnitDistributionMethod"/>
			</owl:Restriction>
		</rdfs:subClassOf>
		<rdfs:subClassOf>
			<owl:Restriction>
				<owl:onProperty rdf:resource="&fibo-fnd-rel-rel;isIssuedBy"/>
				<owl:someValuesFrom rdf:resource="&fibo-sec-fund-civ;UnitIssuer"/>
			</owl:Restriction>
		</rdfs:subClassOf>
		<rdfs:subClassOf>
			<owl:Restriction>
				<owl:onProperty rdf:resource="&fibo-sec-fund-civ;administeredBy"/>
				<owl:someValuesFrom rdf:resource="&fibo-sec-fund-civ;FundAdministrator"/>
			</owl:Restriction>
		</rdfs:subClassOf>
		<rdfs:subClassOf>
			<owl:Restriction>
				<owl:onProperty rdf:resource="&fibo-sec-fund-civ;advisedBy"/>
				<owl:someValuesFrom rdf:resource="&fibo-sec-fund-civ;InvestmentAdvisor"/>
			</owl:Restriction>
		</rdfs:subClassOf>
		<rdfs:subClassOf>
			<owl:Restriction>
				<owl:onProperty rdf:resource="&fibo-sec-fund-civ;distributedBy"/>
				<owl:someValuesFrom rdf:resource="&fibo-sec-fund-civ;FundDistributor"/>
			</owl:Restriction>
		</rdfs:subClassOf>
		<rdfs:subClassOf>
			<owl:Restriction>
				<owl:onProperty rdf:resource="&fibo-sec-fund-civ;fundHasRelatedParty"/>
				<owl:someValuesFrom rdf:resource="&fibo-sec-fund-civ;FundsProcessingParty"/>
			</owl:Restriction>
		</rdfs:subClassOf>
		<rdfs:subClassOf>
			<owl:Restriction>
				<owl:onProperty rdf:resource="&fibo-sec-fund-civ;hasAdditionalInformation"/>
				<owl:someValuesFrom rdf:resource="&fibo-sec-fund-civ;OtherInvestmentFundInformation"/>
			</owl:Restriction>
		</rdfs:subClassOf>
		<rdfs:subClassOf>
			<owl:Restriction>
				<owl:onProperty rdf:resource="&fibo-sec-fund-civ;hasAuditor"/>
				<owl:someValuesFrom rdf:resource="&fibo-sec-fund-civ;FundAuditor"/>
			</owl:Restriction>
		</rdfs:subClassOf>
		<rdfs:subClassOf>
			<owl:Restriction>
				<owl:onProperty rdf:resource="&fibo-sec-fund-civ;hasDataProvider"/>
				<owl:someValuesFrom rdf:resource="&fibo-be-fct-pub;MarketDataProvider"/>
			</owl:Restriction>
		</rdfs:subClassOf>
		<rdfs:subClassOf>
			<owl:Restriction>
				<owl:onProperty rdf:resource="&fibo-sec-fund-civ;hasDepository"/>
				<owl:someValuesFrom rdf:resource="&fibo-sec-fund-civ;FundDepositary"/>
			</owl:Restriction>
		</rdfs:subClassOf>
		<rdfs:subClassOf>
			<owl:Restriction>
				<owl:onProperty rdf:resource="&fibo-sec-fund-civ;hasFundPolicy"/>
				<owl:someValuesFrom rdf:resource="&fibo-sec-fund-civ;FundInvestmentPolicy"/>
			</owl:Restriction>
		</rdfs:subClassOf>
		<rdfs:subClassOf>
			<owl:Restriction>
				<owl:onProperty rdf:resource="&fibo-sec-fund-civ;hasManagementCompany"/>
				<owl:someValuesFrom rdf:resource="&fibo-sec-fund-civ;FundManager"/>
			</owl:Restriction>
		</rdfs:subClassOf>
		<rdfs:subClassOf>
			<owl:Restriction>
				<owl:onProperty rdf:resource="&fibo-sec-fund-civ;hasRelatedFundTerms"/>
				<owl:someValuesFrom rdf:resource="&fibo-sec-fund-civ;FundProcessingTerms"/>
			</owl:Restriction>
		</rdfs:subClassOf>
		<rdfs:subClassOf>
			<owl:Restriction>
				<owl:onProperty rdf:resource="&fibo-sec-fund-civ;hasSubscriptionTerms"/>
				<owl:someValuesFrom rdf:resource="&fibo-sec-fund-civ;FundSubscriptionTerms"/>
			</owl:Restriction>
		</rdfs:subClassOf>
		<rdfs:subClassOf>
			<owl:Restriction>
				<owl:onProperty rdf:resource="&fibo-sec-fund-civ;hasTransferAgent"/>
				<owl:someValuesFrom rdf:resource="&fibo-sec-fund-civ;FundTransferAgent"/>
			</owl:Restriction>
		</rdfs:subClassOf>
		<rdfs:subClassOf>
			<owl:Restriction>
				<owl:onProperty rdf:resource="&fibo-sec-fund-civ;promotedBy"/>
				<owl:someValuesFrom rdf:resource="&fibo-sec-fund-civ;FundPromoter"/>
			</owl:Restriction>
		</rdfs:subClassOf>
		<rdfs:subClassOf>
			<owl:Restriction>
				<owl:onProperty rdf:resource="&fibo-sec-fund-civ;supervisedBy"/>
				<owl:someValuesFrom rdf:resource="&fibo-sec-fund-civ;FundSupervisoryAuthority"/>
			</owl:Restriction>
		</rdfs:subClassOf>
		<rdfs:subClassOf>
			<owl:Restriction>
				<owl:onProperty rdf:resource="&cmns-dsg;isDescribedBy"/>
				<owl:someValuesFrom rdf:resource="&fibo-sec-fund-civ;FundProspectus"/>
			</owl:Restriction>
		</rdfs:subClassOf>
		<cmns-av:explanatoryNote xml:lang="en">From EFAMA DD: The word fund can refer to either an investment pool, umbrella or share class, and is commonly refered to as a collective investment vehicle (can have ISIN or not). The meaning here is for the investment pool (of which an Umbrella fund is also one such) and not to the share class.</cmns-av:explanatoryNote>
	</owl:Class>

</rdf:RDF>