<?xml version="1.0" encoding="UTF-8"?>
<!DOCTYPE rdf:RDF [
	<!ENTITY dct "http://purl.org/dc/terms/">
	<!ENTITY fibo-fnd-acc-cur "https://spec.edmcouncil.org/fibo/ontology/FND/Accounting/CurrencyAmount/">
	<!ENTITY fibo-fnd-accx-assx "https://spec.edmcouncil.org/fibo/ontology/FND/AccountingExt/AssetExtensions/">
	<!ENTITY fibo-fnd-oac-own "https://spec.edmcouncil.org/fibo/ontology/FND/OwnershipAndControl/Ownership/">
	<!ENTITY fibo-fnd-utl-av "https://spec.edmcouncil.org/fibo/ontology/FND/Utilities/AnnotationVocabulary/">
	<!ENTITY owl "http://www.w3.org/2002/07/owl#">
	<!ENTITY rdf "http://www.w3.org/1999/02/22-rdf-syntax-ns#">
	<!ENTITY rdfs "http://www.w3.org/2000/01/rdf-schema#">
	<!ENTITY skos "http://www.w3.org/2004/02/skos/core#">
	<!ENTITY xsd "http://www.w3.org/2001/XMLSchema#">
]>
<rdf:RDF xml:base="https://spec.edmcouncil.org/fibo/ontology/FND/AccountingExt/AssetExtensions/"
	xmlns:dct="http://purl.org/dc/terms/"
	xmlns:fibo-fnd-acc-cur="https://spec.edmcouncil.org/fibo/ontology/FND/Accounting/CurrencyAmount/"
	xmlns:fibo-fnd-accx-assx="https://spec.edmcouncil.org/fibo/ontology/FND/AccountingExt/AssetExtensions/"
	xmlns:fibo-fnd-oac-own="https://spec.edmcouncil.org/fibo/ontology/FND/OwnershipAndControl/Ownership/"
	xmlns:fibo-fnd-utl-av="https://spec.edmcouncil.org/fibo/ontology/FND/Utilities/AnnotationVocabulary/"
	xmlns:owl="http://www.w3.org/2002/07/owl#"
	xmlns:rdf="http://www.w3.org/1999/02/22-rdf-syntax-ns#"
	xmlns:rdfs="http://www.w3.org/2000/01/rdf-schema#"
	xmlns:skos="http://www.w3.org/2004/02/skos/core#"
	xmlns:xsd="http://www.w3.org/2001/XMLSchema#">
	
	<owl:Ontology rdf:about="https://spec.edmcouncil.org/fibo/ontology/FND/AccountingExt/AssetExtensions/">
		<rdfs:label xml:lang="en">AssetExtensions</rdfs:label>
		<dct:abstract>Extensions of concepts in the Asset concept in the main Ownership ontology, where asset is defined as something owned. This ontology covers different categories of asset in that sense, such as physical and real estate (property) assets.</dct:abstract>
		<owl:imports rdf:resource="https://spec.edmcouncil.org/fibo/ontology/FND/Accounting/CurrencyAmount/"/>
		<owl:imports rdf:resource="https://spec.edmcouncil.org/fibo/ontology/FND/OwnershipAndControl/Ownership/"/>
		<owl:imports rdf:resource="https://spec.edmcouncil.org/fibo/ontology/FND/PlacesExt/RealEstate/"/>
		<owl:imports rdf:resource="https://spec.edmcouncil.org/fibo/ontology/FND/Utilities/AnnotationVocabulary/"/>
		<owl:versionIRI rdf:resource="https://spec.edmcouncil.org/fibo/ontology/FND/AccountingExt/AssetExtensions/"/>
		<fibo-fnd-utl-av:hasMaturityLevel rdf:resource="&fibo-fnd-utl-av;Informative"/>
	</owl:Ontology>
	
	<owl:Class rdf:about="&fibo-fnd-accx-assx;MeasurableAsset">
		<rdfs:subClassOf rdf:resource="&fibo-fnd-oac-own;Asset"/>
		<rdfs:subClassOf>
			<owl:Restriction>
				<owl:onProperty rdf:resource="&fibo-fnd-accx-assx;measuredIn"/>
				<owl:someValuesFrom rdf:resource="&fibo-fnd-acc-cur;Currency"/>
			</owl:Restriction>
		</rdfs:subClassOf>
		<rdfs:label xml:lang="en">measurable asset</rdfs:label>
		<skos:definition xml:lang="en">Some asset which is or may be measured monearality in some currency. Editorial Note: This class introduced because the original FIBO model has a property &quot;measured in&quot; (with range of Currency) which is not in FIBO-FND v1.0 and because this lets us use the parent class to define anything as an asset if it is owned whether or not it is measured monetarily. Applications of the concept of Asset to accouting, book-keeping etc where it is measured should use this now term in place of the parent term &quot;Asset&quot;. Note also that the moved property &quot;measured in&quot; is an object property, having a range of Currency.</skos:definition>
	</owl:Class>
	
	<owl:Class rdf:about="&fibo-fnd-accx-assx;PhysicalAsset">
		<rdfs:subClassOf rdf:resource="&fibo-fnd-accx-assx;MeasurableAsset"/>
		<rdfs:label xml:lang="en">physical asset</rdfs:label>
		<skos:definition xml:lang="en">A Physical Thing held by some party and having some value.</skos:definition>
	</owl:Class>
	
	<owl:Class rdf:about="&fibo-fnd-accx-assx;PropertyAsset">
		<rdfs:subClassOf rdf:resource="&fibo-fnd-accx-assx;PhysicalAsset"/>
		<rdfs:subClassOf>
			<owl:Restriction>
				<owl:onProperty rdf:resource="&fibo-fnd-accx-assx;propertyAssetTakesForm"/>
				<owl:someValuesFrom rdf:resource="https://spec.edmcouncil.org/fibo/ontology/FND/Places/Locations/RealEstate"/>
			</owl:Restriction>
		</rdfs:subClassOf>
		<rdfs:label xml:lang="en">property asset</rdfs:label>
		<skos:definition xml:lang="en">A physical property (building) regarded as an asset.</skos:definition>
	</owl:Class>
	
	<owl:ObjectProperty rdf:about="&fibo-fnd-accx-assx;measuredIn">
		<rdfs:label xml:lang="en">measured in</rdfs:label>
		<rdfs:domain rdf:resource="&fibo-fnd-accx-assx;MeasurableAsset"/>
		<rdfs:range rdf:resource="&fibo-fnd-acc-cur;Currency"/>
		<skos:definition xml:lang="en">The currency in which the asset is denominated, measured and / or reported. Explanatory Note: This property was introduced as part of accounting alignment to identify how an asset, when reported for accounting purposes, has some currency in which it may be measured.</skos:definition>
	</owl:ObjectProperty>
	
	<owl:ObjectProperty rdf:about="&fibo-fnd-accx-assx;propertyAssetTakesForm">
		<rdfs:label xml:lang="en">property asset takes form</rdfs:label>
		<rdfs:domain rdf:resource="&fibo-fnd-accx-assx;PropertyAsset"/>
		<rdfs:range rdf:resource="https://spec.edmcouncil.org/fibo/ontology/FND/Places/Locations/RealEstate"/>
		<skos:definition xml:lang="en">The physical form of the Property Asset is Real Estate, also known as Bricks and Mortar.</skos:definition>
	</owl:ObjectProperty>

</rdf:RDF>