<?xml version="1.0" encoding="UTF-8"?>
<!DOCTYPE rdf:RDF [
	<!ENTITY dct "http://purl.org/dc/terms/">
	<!ENTITY fibo-be-le-fbo "https://spec.edmcouncil.org/fibo/BE/LegalEntities/FormalBusinessOrganizations/">
	<!ENTITY fibo-der-der-ex "https://spec.edmcouncil.org/fibo/DER/DerivativesContracts/ExerciseConventions/">
	<!ENTITY fibo-der-der-opt "https://spec.edmcouncil.org/fibo/DER/DerivativesContracts/Options/">
	<!ENTITY fibo-der-etd-eto "https://spec.edmcouncil.org/fibo/DER/ExchangeTradedDerivatives/ExchangeTradedOptions/">
	<!ENTITY fibo-der-etd-ostd "https://spec.edmcouncil.org/fibo/DER/ExchangeTradedDerivatives/OptionsStandardizedTerms/">
	<!ENTITY fibo-der-etd-std "https://spec.edmcouncil.org/fibo/DER/ExchangeTradedDerivatives/DerivativesStandardizedTerms/">
	<!ENTITY fibo-fnd-acc-cur "https://spec.edmcouncil.org/fibo/FND/Accounting/CurrencyAmount/">
	<!ENTITY fibo-fnd-pub-pub "https://spec.edmcouncil.org/fibo/FND/PublicationsExt/Publications/">
	<!ENTITY fibo-fnd-utl-av "https://spec.edmcouncil.org/fibo/FND/Utilities/AnnotationVocabulary/">
	<!ENTITY owl "http://www.w3.org/2002/07/owl#">
	<!ENTITY rdf "http://www.w3.org/1999/02/22-rdf-syntax-ns#">
	<!ENTITY rdfs "http://www.w3.org/2000/01/rdf-schema#">
	<!ENTITY skos "http://www.w3.org/2004/02/skos/core#">
	<!ENTITY xsd "http://www.w3.org/2001/XMLSchema#">
]>
<rdf:RDF xml:base="https://spec.edmcouncil.org/fibo/DER/ExchangeTradedDerivatives/OptionsStandardizedTerms/"
	xmlns:dct="http://purl.org/dc/terms/"
	xmlns:fibo-be-le-fbo="https://spec.edmcouncil.org/fibo/BE/LegalEntities/FormalBusinessOrganizations/"
	xmlns:fibo-der-der-ex="https://spec.edmcouncil.org/fibo/DER/DerivativesContracts/ExerciseConventions/"
	xmlns:fibo-der-der-opt="https://spec.edmcouncil.org/fibo/DER/DerivativesContracts/Options/"
	xmlns:fibo-der-etd-eto="https://spec.edmcouncil.org/fibo/DER/ExchangeTradedDerivatives/ExchangeTradedOptions/"
	xmlns:fibo-der-etd-ostd="https://spec.edmcouncil.org/fibo/DER/ExchangeTradedDerivatives/OptionsStandardizedTerms/"
	xmlns:fibo-der-etd-std="https://spec.edmcouncil.org/fibo/DER/ExchangeTradedDerivatives/DerivativesStandardizedTerms/"
	xmlns:fibo-fnd-acc-cur="https://spec.edmcouncil.org/fibo/FND/Accounting/CurrencyAmount/"
	xmlns:fibo-fnd-pub-pub="https://spec.edmcouncil.org/fibo/FND/PublicationsExt/Publications/"
	xmlns:fibo-fnd-utl-av="https://spec.edmcouncil.org/fibo/FND/Utilities/AnnotationVocabulary/"
	xmlns:owl="http://www.w3.org/2002/07/owl#"
	xmlns:rdf="http://www.w3.org/1999/02/22-rdf-syntax-ns#"
	xmlns:rdfs="http://www.w3.org/2000/01/rdf-schema#"
	xmlns:skos="http://www.w3.org/2004/02/skos/core#"
	xmlns:xsd="http://www.w3.org/2001/XMLSchema#">
	
	<owl:Ontology rdf:about="https://spec.edmcouncil.org/fibo/DER/ExchangeTradedDerivatives/OptionsStandardizedTerms/">
		<rdfs:label xml:lang="en">OptionsStandardizedTerms</rdfs:label>
		<dct:abstract>Standard contractual terms for potential options contracts that an investor may enter into with the derivatives exchange. Includes terms specific to different types of option and different available exercise and delivery arrangements.</dct:abstract>
		<owl:imports rdf:resource="https://spec.edmcouncil.org/fibo/BE/LegalEntities/FormalBusinessOrganizations/"/>
		<owl:imports rdf:resource="https://spec.edmcouncil.org/fibo/DER/DerivativesContracts/ExerciseConventions/"/>
		<owl:imports rdf:resource="https://spec.edmcouncil.org/fibo/DER/DerivativesContracts/Options/"/>
		<owl:imports rdf:resource="https://spec.edmcouncil.org/fibo/DER/ExchangeTradedDerivatives/DerivativesStandardizedTerms/"/>
		<owl:imports rdf:resource="https://spec.edmcouncil.org/fibo/DER/ExchangeTradedDerivatives/ExchangeTradedOptions/"/>
		<owl:imports rdf:resource="https://spec.edmcouncil.org/fibo/FBC/FinancialInstruments/FinancialInstruments/"/>
		<owl:imports rdf:resource="https://spec.edmcouncil.org/fibo/FND/Accounting/CurrencyAmount/"/>
		<owl:imports rdf:resource="https://spec.edmcouncil.org/fibo/FND/PublicationsExt/Publications/"/>
		<owl:imports rdf:resource="https://spec.edmcouncil.org/fibo/FND/Relations/Relations/"/>
		<owl:imports rdf:resource="https://spec.edmcouncil.org/fibo/FND/Utilities/AnnotationVocabulary/"/>
		<owl:imports rdf:resource="https://spec.edmcouncil.org/fibo/MD/DerivativesTemporal/ETOptionsTemporal/"/>
		<owl:versionIRI rdf:resource="https://spec.edmcouncil.org/fibo/DER/ExchangeTradedDerivatives/OptionsStandardizedTerms/"/>
		<fibo-fnd-utl-av:hasMaturityLevel rdf:resource="&fibo-fnd-utl-av;Informative"/>
	</owl:Ontology>
	
	<owl:Class rdf:about="&fibo-der-etd-ostd;OptionsClearingEntity">
		<rdfs:subClassOf rdf:resource="&fibo-be-le-fbo;FormallyConstitutedOrganization"/>
		<rdfs:label xml:lang="en">options clearing entity</rdfs:label>
		<skos:definition xml:lang="en">An entity which is responsible for clearing transactions for put and call options on common stocks and other equity issues, stock indexes, foreign currencies, interest rate composites and single-stock futures.</skos:definition>
		<fibo-fnd-utl-av:explanatoryNote xml:lang="en">e.g. Options Clearing Corporation (US). In Canada the equivalent is In the US, the Options Clearing Corporation defines defaults e.g. lot sizes. This applies to equity options, index options, flex options, yield based options and short dated options. It does not apply to other types of option. Its roles are: 1. Clearing 2. Advocate for sound business practice. Similar to regulator though not officially one. Has a role in risk management Full list from OCC website: OCC clears transactions for put and call options on common stocks and other equity issues, stock indexes, foreign currencies, interest rate composites and single-stock futures</fibo-fnd-utl-av:explanatoryNote>
	</owl:Class>
	
	<owl:Class rdf:about="&fibo-der-etd-ostd;StandardizedCurrencyOptionTermsSet">
		<rdfs:subClassOf rdf:resource="&fibo-der-etd-ostd;StandardizedOptionsTerms"/>
		<rdfs:subClassOf>
			<owl:Restriction>
				<owl:onProperty rdf:resource="&fibo-der-etd-ostd;becomesTermsOf"/>
				<owl:someValuesFrom rdf:resource="&fibo-der-etd-eto;ForeignCurrencyOption"/>
			</owl:Restriction>
		</rdfs:subClassOf>
		<rdfs:label xml:lang="en">standardized currency option terms set</rdfs:label>
		<skos:definition xml:lang="en">Standard terms for a currency optioon contract, determined in advance by the exchange. These will become terms of an individual currency option contract. These may be varied or overridden for individual contracts.</skos:definition>
	</owl:Class>
	
	<owl:Class rdf:about="&fibo-der-etd-ostd;StandardizedEquityOptionTermsSet">
		<rdfs:subClassOf rdf:resource="&fibo-der-etd-ostd;StandardizedOptionsTerms"/>
		<rdfs:subClassOf>
			<owl:Restriction>
				<owl:onProperty rdf:resource="&fibo-der-etd-ostd;becomesTermsOf"/>
				<owl:someValuesFrom rdf:resource="&fibo-der-etd-eto;EquityOption"/>
			</owl:Restriction>
		</rdfs:subClassOf>
		<rdfs:label xml:lang="en">standardized equity option terms set</rdfs:label>
		<skos:definition xml:lang="en">Standard terms for an equity option contract, determined in advance by the exchange. These will become terms of an individual equity option contract. These may be varied or overridden for individual contracts.</skos:definition>
	</owl:Class>
	
	<owl:Class rdf:about="&fibo-der-etd-ostd;StandardizedExerciseTermsSet">
		<rdfs:subClassOf rdf:resource="&fibo-der-etd-ostd;StandardizedOptionsTerms"/>
		<rdfs:subClassOf>
			<owl:Restriction>
				<owl:onProperty rdf:resource="&fibo-der-etd-eto;becomesPartOf"/>
				<owl:someValuesFrom rdf:resource="&fibo-der-etd-eto;OptionInstrumentExerciseTerms"/>
			</owl:Restriction>
		</rdfs:subClassOf>
		<rdfs:subClassOf>
			<owl:Restriction>
				<owl:onProperty rdf:resource="&fibo-der-etd-eto;standardExerciseTermsHasExerciseConvention"/>
				<owl:someValuesFrom rdf:resource="&fibo-der-der-ex;ExerciseDatesConvention"/>
			</owl:Restriction>
		</rdfs:subClassOf>
		<rdfs:subClassOf>
			<owl:Restriction>
				<owl:onProperty rdf:resource="&fibo-der-etd-ostd;specifies"/>
				<owl:someValuesFrom rdf:resource="https://spec.edmcouncil.org/fibo/FBC/FinancialInstruments/FinancialInstruments/FinancialInstrument"/>
			</owl:Restriction>
		</rdfs:subClassOf>
		<rdfs:label xml:lang="en">standardized exercise terms set</rdfs:label>
		<skos:definition xml:lang="en">Standard exercise terms for an option contract, determined in advance by the exchange. These will become exercise terms of an individual option contract. These may be varied or overridden for individual contracts.</skos:definition>
	</owl:Class>
	
	<owl:Class rdf:about="&fibo-der-etd-ostd;StandardizedFuturesOptionTermsSet">
		<rdfs:subClassOf rdf:resource="&fibo-der-etd-ostd;StandardizedOptionsTerms"/>
		<rdfs:subClassOf>
			<owl:Restriction>
				<owl:onProperty rdf:resource="&fibo-der-etd-ostd;becomesTermsOf"/>
				<owl:someValuesFrom rdf:resource="&fibo-der-etd-eto;OptionContractOnFutures"/>
			</owl:Restriction>
		</rdfs:subClassOf>
		<rdfs:label xml:lang="en">standardized futures option terms set</rdfs:label>
		<skos:definition xml:lang="en">Standard terms for a futures options contract, determined in advance by the exchange. These will become terms of an individual futures option contract. These may be varied or overridden for individual contracts.</skos:definition>
	</owl:Class>
	
	<owl:Class rdf:about="&fibo-der-etd-ostd;StandardizedIndexOptionTermsSet">
		<rdfs:subClassOf rdf:resource="&fibo-der-etd-ostd;StandardizedOptionsTerms"/>
		<rdfs:subClassOf>
			<owl:Restriction>
				<owl:onProperty rdf:resource="&fibo-der-etd-ostd;becomesTermsOf"/>
				<owl:someValuesFrom rdf:resource="&fibo-der-etd-eto;ExchangeTradedEquityIndexOption"/>
			</owl:Restriction>
		</rdfs:subClassOf>
		<rdfs:label xml:lang="en">standardized index option terms set</rdfs:label>
		<skos:definition xml:lang="en">Standard terms for an index option contract, determined in advance by the exchange. These will become terms of an individual index option contract. These may be varied or overridden for individual contracts.</skos:definition>
	</owl:Class>
	
	<owl:Class rdf:about="&fibo-der-etd-ostd;StandardizedOptionsTerms">
		<rdfs:subClassOf rdf:resource="https://spec.edmcouncil.org/fibo/FBC/FinancialInstruments/FinancialInstruments/StandardizedTermsSet"/>
		<rdfs:subClassOf>
			<owl:Restriction>
				<owl:onProperty rdf:resource="&fibo-der-etd-ostd;includesFeature"/>
				<owl:onClass rdf:resource="&fibo-der-der-opt;OptionBarrierFeatureTerms"/>
				<owl:maxQualifiedCardinality rdf:datatype="&xsd;nonNegativeInteger">2</owl:maxQualifiedCardinality>
			</owl:Restriction>
		</rdfs:subClassOf>
		<rdfs:subClassOf>
			<owl:Restriction>
				<owl:onProperty rdf:resource="&fibo-der-etd-ostd;becomesTermsOf"/>
				<owl:someValuesFrom rdf:resource="&fibo-der-etd-eto;ExchangeTradedOptionContract"/>
			</owl:Restriction>
		</rdfs:subClassOf>
		<rdfs:subClassOf>
			<owl:Restriction>
				<owl:onProperty rdf:resource="&fibo-der-etd-ostd;definedBy"/>
				<owl:someValuesFrom>
					<owl:Class>
						<owl:unionOf rdf:parseType="Collection">
							<rdf:Description rdf:about="&fibo-der-etd-std;DerivativesExchange">
							</rdf:Description>
							<rdf:Description rdf:about="&fibo-der-etd-ostd;OptionsClearingEntity">
							</rdf:Description>
						</owl:unionOf>
					</owl:Class>
				</owl:someValuesFrom>
			</owl:Restriction>
		</rdfs:subClassOf>
		<rdfs:subClassOf>
			<owl:Restriction>
				<owl:onProperty rdf:resource="&fibo-der-etd-ostd;pricingToBeDeterminedBy"/>
				<owl:someValuesFrom rdf:resource="&fibo-der-etd-std;DerivativesPriceDeterminationMethod"/>
			</owl:Restriction>
		</rdfs:subClassOf>
		<rdfs:label xml:lang="en">standardized options terms</rdfs:label>
		<skos:definition xml:lang="en">A standardized set of terms for an options contract. These are defined by a securities exchange or an options clearing entity. Options contracts issued by the exchange may embody these terms or have equivalent terms which override these.</skos:definition>
	</owl:Class>
	
	<owl:ObjectProperty rdf:about="&fibo-der-etd-ostd;becomesTermsOf">
		<rdfs:label xml:lang="en">becomes terms of</rdfs:label>
		<rdfs:domain rdf:resource="&fibo-der-etd-ostd;StandardizedOptionsTerms"/>
		<rdfs:range rdf:resource="&fibo-der-etd-eto;ExchangeTradedOptionContract"/>
	</owl:ObjectProperty>
	
	<owl:ObjectProperty rdf:about="&fibo-der-etd-ostd;contractSize">
		<rdfs:label xml:lang="en">contract size</rdfs:label>
		<rdfs:domain rdf:resource="&fibo-der-etd-ostd;StandardizedCurrencyOptionTermsSet"/>
		<rdfs:range rdf:resource="&fibo-fnd-acc-cur;MonetaryAmount"/>
		<skos:definition xml:lang="en">The number of units of the currency traded under one Futures Contract.</skos:definition>
	</owl:ObjectProperty>
	
	<owl:DatatypeProperty rdf:about="&fibo-der-etd-ostd;contractSize.1">
		<rdfs:label xml:lang="en">contract size</rdfs:label>
		<rdfs:domain rdf:resource="&fibo-der-etd-ostd;StandardizedEquityOptionTermsSet"/>
		<rdfs:range rdf:resource="&xsd;integer"/>
		<skos:definition xml:lang="en">The number of shares traded under one Option Contract.</skos:definition>
	</owl:DatatypeProperty>
	
	<owl:DatatypeProperty rdf:about="&fibo-der-etd-ostd;contractSize.2">
		<rdfs:label xml:lang="en">contract size</rdfs:label>
		<rdfs:domain rdf:resource="&fibo-der-etd-ostd;StandardizedFuturesOptionTermsSet"/>
		<rdfs:range rdf:resource="&xsd;integer"/>
		<skos:definition xml:lang="en">The number of futures contracts traded under one Futures Option.</skos:definition>
	</owl:DatatypeProperty>
	
	<owl:DatatypeProperty rdf:about="&fibo-der-etd-ostd;contractSize.3">
		<rdfs:label xml:lang="en">contract size</rdfs:label>
		<rdfs:domain rdf:resource="&fibo-der-etd-ostd;StandardizedOptionsTerms"/>
		<rdfs:range rdf:resource="&xsd;integer"/>
		<skos:definition xml:lang="en">Number of underlyers to be in a contract.</skos:definition>
	</owl:DatatypeProperty>
	
	<owl:ObjectProperty rdf:about="&fibo-der-etd-ostd;definedBy">
		<rdfs:subPropertyOf rdf:resource="&fibo-fnd-pub-pub;publishedBy"/>
		<rdfs:label xml:lang="en">defined by</rdfs:label>
		<rdfs:domain rdf:resource="&fibo-der-etd-ostd;StandardizedOptionsTerms"/>
		<rdfs:range>
			<owl:Class>
				<owl:unionOf rdf:parseType="Collection">
					<rdf:Description rdf:about="&fibo-der-etd-std;DerivativesExchange">
					</rdf:Description>
					<rdf:Description rdf:about="&fibo-der-etd-ostd;OptionsClearingEntity">
					</rdf:Description>
				</owl:unionOf>
			</owl:Class>
		</rdfs:range>
	</owl:ObjectProperty>
	
	<owl:ObjectProperty rdf:about="&fibo-der-etd-ostd;includesFeature">
		<rdfs:label xml:lang="en">includes feature</rdfs:label>
		<rdfs:domain rdf:resource="&fibo-der-etd-ostd;StandardizedOptionsTerms"/>
		<rdfs:range rdf:resource="&fibo-der-der-opt;OptionBarrierFeatureTerms"/>
	</owl:ObjectProperty>
	
	<owl:DatatypeProperty rdf:about="&fibo-der-etd-ostd;indexMultiplier">
		<rdfs:label xml:lang="en">index multiplier</rdfs:label>
		<rdfs:domain rdf:resource="&fibo-der-etd-ostd;StandardizedIndexOptionTermsSet"/>
		<rdfs:range rdf:resource="&xsd;decimal"/>
		<skos:definition xml:lang="en">The multiple of the index traded under one Futures contract.</skos:definition>
	</owl:DatatypeProperty>
	
	<owl:ObjectProperty rdf:about="&fibo-der-etd-ostd;optionType">
		<rdfs:label xml:lang="en">option type</rdfs:label>
		<rdfs:domain rdf:resource="&fibo-der-etd-ostd;StandardizedOptionsTerms"/>
		<rdfs:range rdf:resource="&fibo-der-der-opt;OptionTypeSelection"/>
		<skos:definition xml:lang="en">Whether the option will be a call or a put option.</skos:definition>
	</owl:ObjectProperty>
	
	<owl:ObjectProperty rdf:about="&fibo-der-etd-ostd;pricingToBeDeterminedBy">
		<rdfs:label xml:lang="en">pricing to be determined by</rdfs:label>
		<rdfs:domain rdf:resource="&fibo-der-etd-ostd;StandardizedOptionsTerms"/>
		<rdfs:range rdf:resource="&fibo-der-etd-std;DerivativesPriceDeterminationMethod"/>
	</owl:ObjectProperty>
	
	<owl:ObjectProperty rdf:about="&fibo-der-etd-ostd;specifies">
		<rdfs:label xml:lang="en">specifies</rdfs:label>
		<rdfs:domain rdf:resource="&fibo-der-etd-ostd;StandardizedExerciseTermsSet"/>
		<rdfs:range rdf:resource="https://spec.edmcouncil.org/fibo/FBC/FinancialInstruments/FinancialInstruments/FinancialInstrument"/>
	</owl:ObjectProperty>

</rdf:RDF>