<?xml version="1.0" encoding="UTF-8"?>
<rdf:RDF xmlns:xsd="http://www.w3.org/2001/XMLSchema#"
         xmlns:sm="http://www.omg.org/techprocess/ab/SpecificationMetadata/"
         xmlns:fibo-fnd-utl-av="http://www.omg.org/spec/EDMC-FIBO/FND/Utilities/AnnotationVocabulary/"
         xmlns:rdf="http://www.w3.org/1999/02/22-rdf-syntax-ns#"
         xmlns:rdfs="http://www.w3.org/2000/01/rdf-schema#"
         xmlns:owl="http://www.w3.org/2002/07/owl#"
         xmlns:skos="http://www.w3.org/2004/02/skos/core#"
         xmlns:dc="http://purl.org/dc/terms/"
         xml:base="http://www.omg.org/spec/EDMC-SR/FND/Places/Addresses/">

   <owl:Ontology rdf:about="http://www.omg.org/spec/EDMC-SR/FND/Places/Addresses/">
      <owl:imports rdf:resource="http://www.edmcouncil.org/spec/EDMC-SR/FND/Information/InfoCore/"/>
      <owl:imports rdf:resource="http://www.omg.org/spec/EDMC-SR/FND/Places/Locations/"/>
      <owl:imports rdf:resource="http://www.omg.org/spec/EDMC-SR/FND/Places/Countries/"/>
   </owl:Ontology>

   <!--Datatypes-->

<!--Object Properties-->

<owl:ObjectProperty rdf:about="http://www.omg.org/spec/EDMC-SR/FND/Places/Addresses/postalAddressIsIndexTo">
      <skos:definition>The place identified by the Address.</skos:definition>
      <rdfs:subPropertyOf rdf:resource="http://www.omg.org/spec/EDMC-SR/FND/Places/Addresses/isIndexTo"/>
      <rdfs:domain rdf:resource="http://www.omg.org/spec/EDMC-SR/FND/Places/Addresses/PostalAddress"/>
      <rdfs:range rdf:resource="http://www.omg.org/spec/EDMC-SR/FND/Places/Locations/PhysicalLocation"/>
   </owl:ObjectProperty>

   <owl:ObjectProperty rdf:about="http://www.omg.org/spec/EDMC-SR/FND/Places/Addresses/stateAbbreviation">
      <skos:definition>Address element giving the formal abbreviation of the state or province (in federal countries) in which the address is situated.</skos:definition>
      <rdfs:subPropertyOf rdf:resource="http://www.omg.org/spec/EDMC-SR/FND/Places/Addresses/hasAddressComponent"/>
      <rdfs:domain rdf:resource="http://www.omg.org/spec/EDMC-SR/FND/Places/Addresses/Address"/>
      <rdfs:range rdf:resource="http://www.omg.org/spec/EDMC-SR/FND/Places/Addresses/AddressComponent"/>
   </owl:ObjectProperty>

   <owl:ObjectProperty rdf:about="http://www.omg.org/spec/EDMC-SR/FND/Places/Addresses/hasAddressComponent">
      <skos:definition>The postal address has as part of it some distinct textual element which performs some distinct function within the overall address such as referring to some specific physical place, built property feature or post office box.</skos:definition>
      <rdfs:domain rdf:resource="http://www.omg.org/spec/EDMC-SR/FND/Places/Addresses/Address"/>
      <rdfs:range rdf:resource="http://www.omg.org/spec/EDMC-SR/FND/Places/Addresses/AddressComponent"/>
   </owl:ObjectProperty>

   <owl:ObjectProperty rdf:about="http://www.omg.org/spec/EDMC-SR/FND/Places/Addresses/hasCountryName">
      <skos:definition>The name of the country in which the address is situated, in some format which may be recognized in that or other countries.</skos:definition>
      <rdfs:subPropertyOf rdf:resource="http://www.omg.org/spec/EDMC-SR/FND/Places/Addresses/hasAddressComponent"/>
      <rdfs:domain rdf:resource="http://www.omg.org/spec/EDMC-SR/FND/Places/Addresses/Address"/>
      <rdfs:range rdf:resource="http://www.omg.org/spec/EDMC-SR/FND/Places/Addresses/AddressComponent"/>
   </owl:ObjectProperty>

   <owl:ObjectProperty rdf:about="http://www.omg.org/spec/EDMC-SR/FND/Places/Addresses/hasLocality">
      <skos:definition>That part of a written address which uniquely references some town, city or other urban area within the overall address.</skos:definition>
      <rdfs:subPropertyOf rdf:resource="http://www.omg.org/spec/EDMC-SR/FND/Places/Addresses/hasAddressComponent"/>
      <rdfs:domain rdf:resource="http://www.omg.org/spec/EDMC-SR/FND/Places/Addresses/Address"/>
      <rdfs:range rdf:resource="http://www.omg.org/spec/EDMC-SR/FND/Places/Addresses/AddressComponent"/>
   </owl:ObjectProperty>

   <owl:ObjectProperty rdf:about="http://www.omg.org/spec/EDMC-SR/FND/Places/Addresses/hasPOBox">
      <skos:definition>Address element giving the Post Office Box number in the form of digits or letters plus digits.</skos:definition>
      <rdfs:subPropertyOf rdf:resource="http://www.omg.org/spec/EDMC-SR/FND/Places/Addresses/hasAddressComponent"/>
      <rdfs:domain rdf:resource="http://www.omg.org/spec/EDMC-SR/FND/Places/Addresses/Address"/>
      <rdfs:range rdf:resource="http://www.omg.org/spec/EDMC-SR/FND/Places/Addresses/AddressComponent"/>
   </owl:ObjectProperty>

   <owl:ObjectProperty rdf:about="http://www.omg.org/spec/EDMC-SR/FND/Places/Addresses/hasPostalCode">
      <skos:definition>The postal code for an address, in a format recognized by the postal authorities in the country in which the address is situated.</skos:definition>
      <rdfs:subPropertyOf rdf:resource="http://www.omg.org/spec/EDMC-SR/FND/Places/Addresses/hasAddressComponent"/>
      <rdfs:domain rdf:resource="http://www.omg.org/spec/EDMC-SR/FND/Places/Addresses/Address"/>
      <rdfs:range rdf:resource="http://www.omg.org/spec/EDMC-SR/FND/Places/Addresses/AddressComponent"/>
   </owl:ObjectProperty>

   <owl:ObjectProperty rdf:about="http://www.omg.org/spec/EDMC-SR/FND/Places/Addresses/hasStateName">
      <skos:definition>Address element giving the name of the state or province (in federal countries) in which the address is situated.</skos:definition>
      <rdfs:subPropertyOf rdf:resource="http://www.omg.org/spec/EDMC-SR/FND/Places/Addresses/hasAddressComponent"/>
      <rdfs:domain rdf:resource="http://www.omg.org/spec/EDMC-SR/FND/Places/Addresses/Address"/>
      <rdfs:range rdf:resource="http://www.omg.org/spec/EDMC-SR/FND/Places/Addresses/AddressComponent"/>
   </owl:ObjectProperty>

   <owl:ObjectProperty rdf:about="http://www.omg.org/spec/EDMC-SR/FND/Places/Addresses/hasStreetAddress">
      <skos:definition>Address element giving the building name or number and the street in which the address is situated.</skos:definition>
      <rdfs:subPropertyOf rdf:resource="http://www.omg.org/spec/EDMC-SR/FND/Places/Addresses/hasAddressComponent"/>
      <rdfs:domain rdf:resource="http://www.omg.org/spec/EDMC-SR/FND/Places/Addresses/Address"/>
      <rdfs:range rdf:resource="http://www.omg.org/spec/EDMC-SR/FND/Places/Addresses/AddressComponent"/>
   </owl:ObjectProperty>

   <owl:ObjectProperty rdf:about="http://www.omg.org/spec/EDMC-SR/FND/Places/Addresses/isIndexTo">
      <rdfs:subPropertyOf rdf:resource="http://www.omg.org/spec/EDMC-SR/FND/Relations/Relations/identifies"/>
      <rdfs:domain rdf:resource="http://www.omg.org/spec/EDMC-SR/FND/Places/Addresses/Address"/>
      <rdfs:range rdf:resource="http://www.omg.org/spec/EDMC-SR/FND/Places/Locations/Location"/>
   </owl:ObjectProperty>

   <!--Data Properties-->

<owl:DatatypeProperty rdf:about="http://www.omg.org/spec/EDMC-SR/FND/Places/Addresses/addressElementText">
      <rdfs:range rdf:resource="http://www.omg.org/spec/EDMC-SR/FND/Utilities/BusinessFacingTypes/text"/>
   </owl:DatatypeProperty>

   <!--Annotation Properties-->

<!--Classes-->

<owl:Class rdf:about="http://www.omg.org/spec/EDMC-SR/FND/Places/Addresses/Address">
      <rdfs:label>Address</rdfs:label>
      <skos:definition>An address is an index to a location.</skos:definition>
      <skos:editorialNote>Recurrent issues in modeling Address: 1. Address as a self-identifiying literal is distinct form the place addressed; 2. The practical advantage of distinguishing between Address and Address Component. Note that in the US, a general delivery address may be address to the Postmaster for general delivery to that address, or collection. similar for ZA, Aus etc. highway route address Mil address PO Box Rural route addresses Puerto Rico (and RoW)</skos:editorialNote>
      <rdfs:subClassOf rdf:resource="http://www.edmcouncil.org/spec/EDMC-SR/FND/Information/InfoCore/Information"/>
      <rdfs:subClassOf rdf:resource="http://www.edmcouncil.org/spec/EDMC-SR/UO/Lattice/ContinuantThing"/>
      <rdfs:subClassOf rdf:resource="http://www.edmcouncil.org/spec/EDMC-SR/UO/OntologicalDegree/IndependentThing"/>
   </owl:Class>

   <owl:Class rdf:about="http://www.omg.org/spec/EDMC-SR/FND/Places/Addresses/AddressComponent">
      <rdfs:label>Address Component</rdfs:label>
      <skos:definition>A textual element which forms part of some Address. Explanatory Note: This textual element may be used in conjunction with other such elements, or it may comprise a hundred percent of the textual content of the address.</skos:definition>
   </owl:Class>

   <owl:Class rdf:about="http://www.omg.org/spec/EDMC-SR/FND/Places/Addresses/PostcodeArea">
      <rdfs:label>Postcode Area</rdfs:label>
      <skos:definition>An area identified specifically by a postal code or part of a postal code.</skos:definition>
      <skos:editorialNote>Used in risk models etc. - this relates a physical area with some address component (postcode) which identifies that area. Many mortgage pools have this as one of the characteristics of the mortgages in the pool. The postcode area is a recognized risk factor.</skos:editorialNote>
      <rdfs:subClassOf rdf:resource="http://www.edmcouncil.org/spec/EDMC-SR/FND/PlacesExt/Geophysical/GeophysicalLocation"/>
      <rdfs:subClassOf rdf:resource="http://www.omg.org/spec/EDMC-SR/FND/Places/Locations/PhysicalLocation"/>
   </owl:Class>

   <owl:Class rdf:about="http://www.omg.org/spec/EDMC-SR/FND/Places/Addresses/PostalAddress">
      <rdfs:label>Postal Address</rdfs:label>
      <skos:definition>A physical and postal address where communications can be addressed, papers served or representatives located for any kind of business entity or legal entity.</skos:definition>
      <skos:editorialNote>Alternative definition (FDTF Address Reviews Aug/Sept 2011): An index to a location to which physical communications may be delivered. Editorial note: There are existing international standards for defining this structure. This should be found and used. The current model is a place holder until that material can be located and included.</skos:editorialNote>
      <rdfs:subClassOf rdf:resource="http://www.edmcouncil.org/spec/EDMC-SR/FND/Relative/SetMembership/Set"/>
      <rdfs:subClassOf rdf:resource="http://www.omg.org/spec/EDMC-SR/FND/Places/Addresses/Address"/>
   </owl:Class>

   <!--Individuals-->

</rdf:RDF>