<?xml version="1.0" encoding="UTF-8"?>
<rdf:RDF xmlns:xsd="http://www.w3.org/2001/XMLSchema#"
         xmlns:sm="http://www.omg.org/techprocess/ab/SpecificationMetadata/"
         xmlns:fibo-fnd-utl-av="http://www.omg.org/spec/EDMC-FIBO/FND/Utilities/AnnotationVocabulary/"
         xmlns:rdf="http://www.w3.org/1999/02/22-rdf-syntax-ns#"
         xmlns:rdfs="http://www.w3.org/2000/01/rdf-schema#"
         xmlns:owl="http://www.w3.org/2002/07/owl#"
         xmlns:skos="http://www.w3.org/2004/02/skos/core#"
         xmlns:dc="http://purl.org/dc/terms/"
         xml:base="http://www.edmcouncil.org/spec/EDMC-SR/FND/Accounting/AssetExtensions/">

   <owl:Ontology rdf:about="http://www.edmcouncil.org/spec/EDMC-SR/FND/Accounting/AssetExtensions/">
      <owl:imports rdf:resource="http://www.omg.org/spec/EDMC-SR/FND/Places/Locations/"/>
      <owl:imports rdf:resource="http://www.omg.org/spec/EDMC-SR/FND/Accounting/CurrencyAmount/"/>
      <owl:imports rdf:resource="http://www.omg.org/spec/EDMC-SR/FND/OwnershipAndControl/Ownership/"/>
      <owl:imports rdf:resource="http://www.edmcouncil.org/spec/EDMC-SR/FND/Physical/Physical/"/>
   </owl:Ontology>

   <!--Datatypes-->

<!--Object Properties-->

<owl:ObjectProperty rdf:about="http://www.edmcouncil.org/spec/EDMC-SR/FND/Accounting/AssetExtensions/physicalAssetTakesForm">
      <skos:definition>The individual thing which itself makes up the Asset.</skos:definition>
      <rdfs:subPropertyOf rdf:resource="http://www.omg.org/spec/EDMC-SR/FND/OwnershipAndControl/Ownership/asssetTakesForm"/>
      <rdfs:domain rdf:resource="http://www.edmcouncil.org/spec/EDMC-SR/FND/Accounting/AssetExtensions/PhysicalAsset"/>
      <rdfs:range rdf:resource="http://www.edmcouncil.org/spec/EDMC-SR/FND/Physical/Physical/DiscretePhysicalThing"/>
   </owl:ObjectProperty>

   <owl:ObjectProperty rdf:about="http://www.edmcouncil.org/spec/EDMC-SR/FND/Accounting/AssetExtensions/measuredIn">
      <skos:definition>The currency in which the asset is denominated, measured and / or reported. Explanatory Note: This property was introduced as part of accounting alignment to identify how an asset, when reported for accounting purposes, has some currency in which it may be measured.</skos:definition>
      <rdfs:domain rdf:resource="http://www.edmcouncil.org/spec/EDMC-SR/FND/Accounting/AssetExtensions/MeasurableAsset"/>
      <rdfs:range rdf:resource="http://www.omg.org/spec/EDMC-SR/FND/Accounting/CurrencyAmount/Currency"/>
   </owl:ObjectProperty>

   <owl:ObjectProperty rdf:about="http://www.edmcouncil.org/spec/EDMC-SR/FND/Accounting/AssetExtensions/propertyAssetTakesForm">
      <skos:definition>The physical form of the Property Asset is Real Estate, also known as Bricks and Mortar.</skos:definition>
      <rdfs:subPropertyOf rdf:resource="http://www.edmcouncil.org/spec/EDMC-SR/FND/Accounting/AssetExtensions/physicalAssetTakesForm"/>
      <rdfs:domain rdf:resource="http://www.edmcouncil.org/spec/EDMC-SR/FND/Accounting/AssetExtensions/PropertyAsset"/>
      <rdfs:range rdf:resource="http://www.omg.org/spec/EDMC-SR/FND/Places/Locations/RealEstate"/>
   </owl:ObjectProperty>

   <!--Data Properties-->

<!--Annotation Properties-->

<!--Classes-->

<owl:Class rdf:about="http://www.edmcouncil.org/spec/EDMC-SR/FND/Accounting/AssetExtensions/MeasurableAsset">
      <rdfs:label>Measurable Asset</rdfs:label>
      <skos:definition>Some asset which is or may be measured monearality in some currency. Editorial Note: This class introduced because the original FIBO model has a property "measured in" (with range of Currency) which is not in FIBO-FND v1.0 and because this lets us use the parent class to define anything as an asset if it is owned whether or not it is measured monetarily. Applications of the concept of Asset to accouting, book-keeping etc where it is measured should use this now term in place of the parent term "Asset". Note also that the moved property "measured in" is an object property, having a range of Currency.</skos:definition>
      <rdfs:subClassOf rdf:resource="http://www.omg.org/spec/EDMC-SR/FND/OwnershipAndControl/Ownership/Asset"/>
   </owl:Class>

   <owl:Class rdf:about="http://www.edmcouncil.org/spec/EDMC-SR/FND/Accounting/AssetExtensions/PhysicalAsset">
      <rdfs:label>Physical Asset</rdfs:label>
      <skos:definition>A Physical Thing held by some party and having some value.</skos:definition>
      <rdfs:subClassOf rdf:resource="http://www.edmcouncil.org/spec/EDMC-SR/FND/Accounting/AssetExtensions/MeasurableAsset"/>
   </owl:Class>

   <owl:Class rdf:about="http://www.edmcouncil.org/spec/EDMC-SR/FND/Accounting/AssetExtensions/PropertyAsset">
      <rdfs:label>Property Asset</rdfs:label>
      <skos:definition>A physical property (building) regarded as an asset.</skos:definition>
      <rdfs:subClassOf rdf:resource="http://www.edmcouncil.org/spec/EDMC-SR/FND/Accounting/AssetExtensions/PhysicalAsset"/>
   </owl:Class>

   <!--Individuals-->

</rdf:RDF>