<?xml version="1.0" encoding="UTF-8"?>
  
<!DOCTYPE rdf:RDF [
    <!ENTITY fibo-sec-dbt-ab-spv "http://spec.edmcouncil.org/fibo/red/sec/debt/asset-backed/asset-backed-spv/">
    <!ENTITY fibo-be-fct-spv "http://spec.edmcouncil.org/fibo/red/be/functional-entities-ext/spv/">
    <!ENTITY fibo-sec-sec-pls "http://spec.edmcouncil.org/fibo/red/sec/securities/pools/">
    <!ENTITY fibo-fnd-utl-bt "http://spec.edmcouncil.org/fibo/red/fnd/utilities/business-facing-types/">
]>

<rdf:RDF xmlns:xsd="http://www.w3.org/2001/XMLSchema#"
         xmlns:sm="http://www.omg.org/techprocess/ab/SpecificationMetadata/"
         xmlns:xs="http://www.w3.org/2001/XMLSchema"
         xmlns:fibo-fnd-utl-av="http://www.omg.org/spec/EDMC-FIBO/FND/Utilities/AnnotationVocabulary/"
         xmlns:rdf="http://www.w3.org/1999/02/22-rdf-syntax-ns#"
         xmlns:rdfs="http://www.w3.org/2000/01/rdf-schema#"
         xmlns:owl="http://www.w3.org/2002/07/owl#"
         xmlns:skos="http://www.w3.org/2004/02/skos/core#"
         xmlns:dc="http://purl.org/dc/terms/"
         xml:base="http://spec.edmcouncil.org/fibo/red/sec/debt/asset-backed/asset-backed-spv/">

   <owl:Ontology rdf:about="http://spec.edmcouncil.org/fibo/red/sec/debt/asset-backed/asset-backed-spv/">
      <owl:imports rdf:resource="http://spec.edmcouncil.org/fibo/red/be/functional-entities-ext/spv/"/>
      <owl:imports rdf:resource="http://spec.edmcouncil.org/fibo/red/sec/securities/pools/"/>
      <owl:imports rdf:resource="http://spec.edmcouncil.org/fibo/red/fnd/utilities/business-facing-types/"/>
   </owl:Ontology>


  <!--
    ///////////////////////////////////////////////////////////////////////////////////////
    //
    // Datatypes
    //
    ///////////////////////////////////////////////////////////////////////////////////////
    -->



  <!--
    ///////////////////////////////////////////////////////////////////////////////////////
    //
    // Object Properties
    //
    ///////////////////////////////////////////////////////////////////////////////////////
    -->


<owl:ObjectProperty rdf:about="&fibo-sec-dbt-ab-spv;holds">
      <rdfs:label>holds</rdfs:label>
      <skos:definition>The Debt Special Purpose Vehicle holds assets in the form of a debt pool.</skos:definition>
      <rdfs:subPropertyOf rdf:resource="&fibo-sec-sec-pls;sPVHoldsPool"/>
      <rdfs:domain rdf:resource="&fibo-sec-dbt-ab-spv;DebtSPV"/>
      <rdfs:range rdf:resource="&fibo-sec-sec-pls;DebtPool"/>
   </owl:ObjectProperty>


  <!--
    ///////////////////////////////////////////////////////////////////////////////////////
    //
    // Data Properties
    //
    ///////////////////////////////////////////////////////////////////////////////////////
    -->


<owl:DatatypeProperty rdf:about="&fibo-sec-dbt-ab-spv;isREMIC">
      <rdfs:label>is r e m i c</rdfs:label>
      <skos:definition>Whether the SPV is set up and registered as a Real Estate Mortgage Investment Conduit (REMIC). REMICs are a type of special purpose vehicle used for the pooling of mortgage loans and issuance of mortgage-backed securities. They are defined under the United States Internal Revenue Code (Tax Reform Act of 1986), and are the typical vehicle of choice for the securitization of residential mortgages in the US.</skos:definition>
      <rdfs:range rdf:resource="&fibo-fnd-utl-bt;yesOrNo"/>
   </owl:DatatypeProperty>

   <owl:DatatypeProperty rdf:about="&fibo-sec-dbt-ab-spv;purpose">
      <rdfs:label>purpose</rdfs:label>
      <skos:definition>The purpose for which the Debt SPV is set up is for the issue of debt securities such as structured finance.</skos:definition>
      <rdfs:range rdf:resource="&fibo-be-fct-spv;SPVPurposeSelection"/>
   </owl:DatatypeProperty>


  <!--
    ///////////////////////////////////////////////////////////////////////////////////////
    //
    // Annotation Properties
    //
    ///////////////////////////////////////////////////////////////////////////////////////
    -->



  <!--
    ///////////////////////////////////////////////////////////////////////////////////////
    //
    // Classes
    //
    ///////////////////////////////////////////////////////////////////////////////////////
    -->


<owl:Class rdf:about="&fibo-sec-dbt-ab-spv;DebtSPV">
      <rdfs:label>debt s p v</rdfs:label>
      <skos:definition>A Special Purpose Vehicle (SPV) set up specifically to issue a debt security or securities. It is set up by a company or a group of companies to create instruments that are off the company's balance sheet.</skos:definition>
      <rdfs:subClassOf rdf:resource="&fibo-be-fct-spv;SpecialPurposeVehicle"/>
   </owl:Class>


  <!--
    ///////////////////////////////////////////////////////////////////////////////////////
    //
    // Individuals
    //
    ///////////////////////////////////////////////////////////////////////////////////////
    -->


</rdf:RDF>