<?xml version="1.0" encoding="UTF-8"?>
<!DOCTYPE rdf:RDF [
	<!ENTITY fibo-der-der-ex "https://spec.edmcouncil.org/fibo/DER/DerivativesContracts/ExerciseConventions/">
	<!ENTITY fibo-fnd-agr-ctr "https://spec.edmcouncil.org/fibo/FND/Agreements/Contracts/">
	<!ENTITY fibo-fnd-arrx-qua "https://spec.edmcouncil.org/fibo/FND/Arrangements/Quantities/">
	<!ENTITY fibo-fnd-dt-fd "https://spec.edmcouncil.org/fibo/FND/DatesAndTimes/FinancialDates/">
	<!ENTITY fibo-fnd-math-amt "https://spec.edmcouncil.org/fibo/FND/Math/Amounts/">
	<!ENTITY fibo-fnd-math-math "https://spec.edmcouncil.org/fibo/FND/Math/Math/">
	<!ENTITY fibo-fnd-occ-ev "https://spec.edmcouncil.org/fibo/FND/Occurrent/Events/">
	<!ENTITY fibo-fnd-rel-rel "https://spec.edmcouncil.org/fibo/FND/Relations/Relations/">
	<!ENTITY fibo-fnd-tim-tim "https://spec.edmcouncil.org/fibo/FND/Time/Time/">
	<!ENTITY fibo-fnd-utl-av "https://spec.edmcouncil.org/fibo/FND/Utilities/AnnotationVocabulary/">
	<!ENTITY fibo-fnd-utl-val "https://spec.edmcouncil.org/fibo/FND/Utilities/Values/">
	<!ENTITY fibo-md-dbt-aly "https://spec.edmcouncil.org/fibo/MD/DebtTemporal/DebtAnalytics/">
	<!ENTITY fibo-md-dbt-py "https://spec.edmcouncil.org/fibo/MD/DebtTemporal/DebtPricingYields/">
	<!ENTITY fibo-md-tem-ins "https://spec.edmcouncil.org/fibo/MD/TemporalCore/InstrumentTemporalTerms/">
	<!ENTITY fibo-sec-dbt-dbt-cft "https://spec.edmcouncil.org/fibo/SEC/Debt/DebtFoundations/DebtCashflowTerms/">
	<!ENTITY fibo-sec-dbt-dbt-dbt "https://spec.edmcouncil.org/fibo/SEC/Debt/DebtFoundations/DebtInstruments/">
	<!ENTITY fibo-sec-sec-schx "https://spec.edmcouncil.org/fibo/SEC/Securities/SchedulesExt/">
	<!ENTITY fibo-uo-lat "https://spec.edmcouncil.org/fibo/UO/Lattice/">
	<!ENTITY owl "http://www.w3.org/2002/07/owl#">
	<!ENTITY rdf "http://www.w3.org/1999/02/22-rdf-syntax-ns#">
	<!ENTITY rdfs "http://www.w3.org/2000/01/rdf-schema#">
	<!ENTITY skos "http://www.w3.org/2004/02/skos/core#">
	<!ENTITY terms "http://purl.org/dc/terms/">
	<!ENTITY xsd "http://www.w3.org/2001/XMLSchema#">
]>
<rdf:RDF
	xml:base="https://spec.edmcouncil.org/fibo/SEC/Debt/DebtFoundations/DebtCashflowTerms/"
	xmlns:fibo-der-der-ex="https://spec.edmcouncil.org/fibo/DER/DerivativesContracts/ExerciseConventions/"
	xmlns:fibo-fnd-agr-ctr="https://spec.edmcouncil.org/fibo/FND/Agreements/Contracts/"
	xmlns:fibo-fnd-arrx-qua="https://spec.edmcouncil.org/fibo/FND/Arrangements/Quantities/"
	xmlns:fibo-fnd-dt-fd="https://spec.edmcouncil.org/fibo/FND/DatesAndTimes/FinancialDates/"
	xmlns:fibo-fnd-math-amt="https://spec.edmcouncil.org/fibo/FND/Math/Amounts/"
	xmlns:fibo-fnd-math-math="https://spec.edmcouncil.org/fibo/FND/Math/Math/"
	xmlns:fibo-fnd-occ-ev="https://spec.edmcouncil.org/fibo/FND/Occurrent/Events/"
	xmlns:fibo-fnd-rel-rel="https://spec.edmcouncil.org/fibo/FND/Relations/Relations/"
	xmlns:fibo-fnd-tim-tim="https://spec.edmcouncil.org/fibo/FND/Time/Time/"
	xmlns:fibo-fnd-utl-av="https://spec.edmcouncil.org/fibo/FND/Utilities/AnnotationVocabulary/"
	xmlns:fibo-fnd-utl-val="https://spec.edmcouncil.org/fibo/FND/Utilities/Values/"
	xmlns:fibo-md-dbt-aly="https://spec.edmcouncil.org/fibo/MD/DebtTemporal/DebtAnalytics/"
	xmlns:fibo-md-dbt-py="https://spec.edmcouncil.org/fibo/MD/DebtTemporal/DebtPricingYields/"
	xmlns:fibo-md-tem-ins="https://spec.edmcouncil.org/fibo/MD/TemporalCore/InstrumentTemporalTerms/"
	xmlns:fibo-sec-dbt-dbt-cft="https://spec.edmcouncil.org/fibo/SEC/Debt/DebtFoundations/DebtCashflowTerms/"
	xmlns:fibo-sec-dbt-dbt-dbt="https://spec.edmcouncil.org/fibo/SEC/Debt/DebtFoundations/DebtInstruments/"
	xmlns:fibo-sec-sec-schx="https://spec.edmcouncil.org/fibo/SEC/Securities/SchedulesExt/"
	xmlns:fibo-uo-lat="https://spec.edmcouncil.org/fibo/UO/Lattice/"
	xmlns:owl="http://www.w3.org/2002/07/owl#"
	xmlns:rdf="http://www.w3.org/1999/02/22-rdf-syntax-ns#"
	xmlns:rdfs="http://www.w3.org/2000/01/rdf-schema#"
	xmlns:skos="http://www.w3.org/2004/02/skos/core#"
	xmlns:terms="http://purl.org/dc/terms/"
	xmlns:xsd="http://www.w3.org/2001/XMLSchema#">
	
	<owl:Ontology
		rdf:about="https://spec.edmcouncil.org/fibo/SEC/Debt/DebtFoundations/DebtCashflowTerms/">
		<rdfs:label>DebtCashflowTerms</rdfs:label>
		<owl:imports
			rdf:resource="http://www.w3.org/2004/02/skos/core"/>
		<owl:imports
			rdf:resource="https://spec.edmcouncil.org/fibo/DER/DerivativesContracts/ExerciseConventions/"/>
		<owl:imports
			rdf:resource="https://spec.edmcouncil.org/fibo/FBC/DebtAndEquities/Debt/"/>
		<owl:imports
			rdf:resource="https://spec.edmcouncil.org/fibo/FND/Agreements/Contracts/"/>
		<owl:imports
			rdf:resource="https://spec.edmcouncil.org/fibo/FND/Arrangements/Quantities/"/>
		<owl:imports
			rdf:resource="https://spec.edmcouncil.org/fibo/FND/DatesAndTimes/FinancialDates/"/>
		<owl:imports
			rdf:resource="https://spec.edmcouncil.org/fibo/FND/Math/Amounts/"/>
		<owl:imports
			rdf:resource="https://spec.edmcouncil.org/fibo/FND/Math/Math/"/>
		<owl:imports
			rdf:resource="https://spec.edmcouncil.org/fibo/FND/Relations/Relations/"/>
		<owl:imports
			rdf:resource="https://spec.edmcouncil.org/fibo/FND/Time/Time/"/>
		<owl:imports
			rdf:resource="https://spec.edmcouncil.org/fibo/FND/Utilities/AnnotationVocabulary/"/>
		<owl:imports
			rdf:resource="https://spec.edmcouncil.org/fibo/FND/Utilities/Values/"/>
		<owl:imports
			rdf:resource="https://spec.edmcouncil.org/fibo/IND/Indicators/Indicators/"/>
		<owl:imports
			rdf:resource="https://spec.edmcouncil.org/fibo/MD/DebtTemporal/DebtAnalytics/"/>
		<owl:imports
			rdf:resource="https://spec.edmcouncil.org/fibo/MD/DebtTemporal/DebtPricingYields/"/>
		<owl:imports
			rdf:resource="https://spec.edmcouncil.org/fibo/MD/TemporalCore/InstrumentTemporalTerms/"/>
		<owl:imports
			rdf:resource="https://spec.edmcouncil.org/fibo/SEC/Debt/DebtFoundations/DebtInstruments/"/>
		<owl:imports
			rdf:resource="https://spec.edmcouncil.org/fibo/SEC/Securities/SchedulesExt/"/>
	</owl:Ontology>
	
	<owl:Class
		rdf:about="&fibo-sec-dbt-dbt-cft;Accreting">
		<rdfs:subClassOf
			rdf:resource="&fibo-sec-dbt-dbt-cft;AmortizationType"/>
		<rdfs:label>accreting</rdfs:label>
	</owl:Class>
	
	<owl:Class
		rdf:about="&fibo-sec-dbt-dbt-cft;AmortizationType">
		<rdfs:label>amortization type</rdfs:label>
		<skos:definition>The different types of principal payments applicable to a debt security.</skos:definition>
	</owl:Class>
	
	<owl:Class
		rdf:about="&fibo-sec-dbt-dbt-cft;Base">
		<rdfs:subClassOf
			rdf:resource="&fibo-fnd-math-math;FormulaArgument"/>
		<rdfs:subClassOf>
			<owl:Restriction>
				<owl:maxQualifiedCardinality
					rdf:datatype="&xsd;nonNegativeInteger">1</owl:maxQualifiedCardinality>
				<owl:onClass
					rdf:resource="&fibo-fnd-utl-val;IntegerValue"/>
				<owl:onProperty
					rdf:resource="&fibo-sec-dbt-dbt-cft;roundingDecimalPlaces"/>
			</owl:Restriction>
		</rdfs:subClassOf>
		<rdfs:subClassOf>
			<owl:Restriction>
				<owl:maxQualifiedCardinality
					rdf:datatype="&xsd;nonNegativeInteger">1</owl:maxQualifiedCardinality>
				<owl:onClass
					rdf:resource="&fibo-fnd-utl-val;IntegerValue"/>
				<owl:onProperty
					rdf:resource="&fibo-sec-dbt-dbt-cft;truncatingDecimalPlaces"/>
			</owl:Restriction>
		</rdfs:subClassOf>
		<rdfs:subClassOf>
			<owl:Restriction>
				<owl:onProperty
					rdf:resource="&fibo-fnd-math-math;hasOperand"/>
				<owl:someValuesFrom
					rdf:resource="https://spec.edmcouncil.org/fibo/IND/Indicators/Indicators/MarketRate"/>
			</owl:Restriction>
		</rdfs:subClassOf>
		<rdfs:label>base</rdfs:label>
		<skos:definition>The variable to which an additional Margin amount is added to get the Interest amount.</skos:definition>
	</owl:Class>
	
	<owl:Class
		rdf:about="&fibo-sec-dbt-dbt-cft;BondContinuousCallType">
		<rdfs:label>bond continuous call type</rdfs:label>
		<terms:description>Bond may be called at any time</terms:description>
	</owl:Class>
	
	<owl:Class
		rdf:about="&fibo-sec-dbt-dbt-cft;CalendarType">
		<rdfs:label>calendar day type</rdfs:label>
		<owl:equivalentClass>
			<owl:Class>
				<owl:unionOf>
					<rdf:Description>
						<rdf:first
							rdf:resource="&fibo-fnd-tim-tim;BusinessDay"/>
						<rdf:rest>
							<rdf:Description>
								<rdf:first
									rdf:resource="&fibo-fnd-tim-tim;CalendarDay"/>
								<rdf:rest
									rdf:resource="&rdf;nil"/>
							</rdf:Description>
						</rdf:rest>
					</rdf:Description>
				</owl:unionOf>
			</owl:Class>
		</owl:equivalentClass>
		<skos:definition>Calendar is defined in terms of either a Calendar Day or a Business Day.</skos:definition>
	</owl:Class>
	
	<owl:Class
		rdf:about="&fibo-sec-dbt-dbt-cft;DebtCallTerms">
		<rdfs:subClassOf
			rdf:resource="https://spec.edmcouncil.org/fibo/FBC/DebtAndEquities/Debt/PrincipalRepaymentTerms"/>
		<rdfs:label>debt call terms</rdfs:label>
	</owl:Class>
	
	<owl:Class
		rdf:about="&fibo-sec-dbt-dbt-cft;DebtSecurityInterestPaymentTerms">
		<rdfs:subClassOf
			rdf:resource="https://spec.edmcouncil.org/fibo/FBC/DebtAndEquities/Debt/InterestPaymentTerms"/>
		<rdfs:subClassOf>
			<owl:Restriction>
				<owl:maxQualifiedCardinality
					rdf:datatype="&xsd;nonNegativeInteger">12</owl:maxQualifiedCardinality>
				<owl:onClass
					rdf:resource="&fibo-fnd-utl-val;DayMonthValue"/>
				<owl:onProperty
					rdf:resource="&fibo-sec-dbt-dbt-cft;interestPaymentDayAndMonth"/>
			</owl:Restriction>
		</rdfs:subClassOf>
		<rdfs:subClassOf>
			<owl:Restriction>
				<owl:minQualifiedCardinality
					rdf:datatype="&xsd;nonNegativeInteger">1</owl:minQualifiedCardinality>
				<owl:onClass
					rdf:resource="&fibo-fnd-utl-val;DayMonthValue"/>
				<owl:onProperty
					rdf:resource="&fibo-sec-dbt-dbt-cft;interestPaymentDayAndMonth"/>
			</owl:Restriction>
		</rdfs:subClassOf>
		<rdfs:subClassOf>
			<owl:Restriction>
				<owl:onProperty
					rdf:resource="&fibo-sec-dbt-dbt-cft;hasAccrualBasis"/>
				<owl:someValuesFrom
					rdf:resource="&fibo-sec-dbt-dbt-dbt;DayCountBasis"/>
			</owl:Restriction>
		</rdfs:subClassOf>
		<rdfs:label>debt security interest payment terms</rdfs:label>
		<skos:definition>Terms defining the interest or Coupon to be paid on a security.</skos:definition>
	</owl:Class>
	
	<owl:Class
		rdf:about="&fibo-sec-dbt-dbt-cft;ExtendableMaturityRedemptionTermsSet">
		<rdfs:subClassOf
			rdf:resource="https://spec.edmcouncil.org/fibo/FBC/DebtAndEquities/Debt/PrincipalRepaymentTerms"/>
		<rdfs:label>extendable maturity redemption terms set</rdfs:label>
		<skos:definition>Terms for the redemption of a security with extendable maturity.</skos:definition>
	</owl:Class>
	
	<owl:Class
		rdf:about="&fibo-sec-dbt-dbt-cft;FactorCalculationFormula">
		<rdfs:subClassOf
			rdf:resource="&fibo-fnd-math-math;Formula"/>
		<rdfs:label>factor calculation formula</rdfs:label>
		<skos:definition>Formula for the determination of some variable factor which is then used in subsequent calculations. The result of such a formula is a parameter referred to by another formula.</skos:definition>
		<fibo-fnd-utl-av:explanatoryNote>Examples include the formula for determining the Factor for an Inflation Bond, which may then be used in calculation of interest payments, principal repayments or both. It is referred to separately and may be determined by a different party to the party which determines the factor itself. Consensus:Review</fibo-fnd-utl-av:explanatoryNote>
	</owl:Class>
	
	<owl:Class
		rdf:about="&fibo-sec-dbt-dbt-cft;InterestCalculationExpression">
		<rdfs:subClassOf
			rdf:resource="&fibo-fnd-math-math;FormulaExpression"/>
		<rdfs:subClassOf>
			<owl:Restriction>
				<owl:onProperty
					rdf:resource="&fibo-sec-dbt-dbt-cft;hasBaseParameter"/>
				<owl:someValuesFrom
					rdf:resource="&fibo-sec-dbt-dbt-cft;Base"/>
			</owl:Restriction>
		</rdfs:subClassOf>
		<rdfs:subClassOf>
			<owl:Restriction>
				<owl:onProperty
					rdf:resource="&fibo-sec-dbt-dbt-cft;hasMarginParameter"/>
				<owl:someValuesFrom
					rdf:resource="&fibo-sec-dbt-dbt-cft;Margin"/>
			</owl:Restriction>
		</rdfs:subClassOf>
		<rdfs:label>interest calculation expression</rdfs:label>
		<skos:definition>How the Formula is expressed i.e. the Right Hand Side of the Formula. This has separate parameters for Base and Margin. The overall Expression is not modeled but may be additionally described in a free form text field.</skos:definition>
	</owl:Class>
	
	<owl:Class
		rdf:about="&fibo-sec-dbt-dbt-cft;InterestCalculationFormula">
		<rdfs:subClassOf
			rdf:resource="&fibo-fnd-math-math;Formula"/>
		<rdfs:subClassOf>
			<owl:Restriction>
				<owl:onProperty
					rdf:resource="&fibo-fnd-math-math;hasExpression"/>
				<owl:someValuesFrom
					rdf:resource="&fibo-sec-dbt-dbt-cft;InterestCalculationExpression"/>
			</owl:Restriction>
		</rdfs:subClassOf>
		<rdfs:subClassOf>
			<owl:Restriction>
				<owl:onProperty
					rdf:resource="&fibo-fnd-math-math;hasSubject"/>
				<owl:someValuesFrom
					rdf:resource="&fibo-sec-dbt-dbt-cft;InterestCalculationSubject"/>
			</owl:Restriction>
		</rdfs:subClassOf>
		<rdfs:label>interest calculation formula</rdfs:label>
		<skos:definition>Formula for calculation of Interest.</skos:definition>
	</owl:Class>
	
	<owl:Class
		rdf:about="&fibo-sec-dbt-dbt-cft;InterestCalculationSubject">
		<rdfs:subClassOf
			rdf:resource="&fibo-fnd-math-math;FormulaSubject"/>
		<rdfs:subClassOf>
			<owl:Restriction>
				<owl:onProperty
					rdf:resource="&fibo-sec-dbt-dbt-cft;subjectIs"/>
				<owl:someValuesFrom
					rdf:resource="&fibo-sec-dbt-dbt-cft;SecuritizedDebtInterest"/>
			</owl:Restriction>
		</rdfs:subClassOf>
		<rdfs:label>interest calculation subject</rdfs:label>
		<skos:definition>The Subject or Left Hand Side of an Interest Calculation Formula. This is by definition the Interest amount.</skos:definition>
	</owl:Class>
	
	<owl:Class
		rdf:about="&fibo-sec-dbt-dbt-cft;InterestOnly">
		<rdfs:subClassOf
			rdf:resource="&fibo-sec-dbt-dbt-cft;AmortizationType"/>
		<rdfs:label>interest only</rdfs:label>
	</owl:Class>
	
	<owl:Class
		rdf:about="&fibo-sec-dbt-dbt-cft;Margin">
		<rdfs:subClassOf
			rdf:resource="&fibo-fnd-math-math;FormulaArgument"/>
		<rdfs:label>margin</rdfs:label>
		<skos:definition>The parameter of the Expression which is added to the Base to get the Interest amount.</skos:definition>
	</owl:Class>
	
	<owl:Class
		rdf:about="&fibo-sec-dbt-dbt-cft;NonTradableDebtInterestTerms">
		<rdfs:subClassOf
			rdf:resource="https://spec.edmcouncil.org/fibo/FBC/DebtAndEquities/Debt/InterestPaymentTerms"/>
		<rdfs:label>non tradable debt interest terms</rdfs:label>
		<skos:definition>Terms for payment of interest on debt instruments that are not traded securities, i.e. over the counter, bilateral paper.</skos:definition>
	</owl:Class>
	
	<owl:Class
		rdf:about="&fibo-sec-dbt-dbt-cft;NotificationFeature">
		<rdfs:subClassOf
			rdf:resource="https://spec.edmcouncil.org/fibo/FBC/DebtAndEquities/Debt/PrincipalRepaymentTerms"/>
		<rdfs:label>notification feature</rdfs:label>
	</owl:Class>
	
	<owl:Class
		rdf:about="&fibo-sec-dbt-dbt-cft;PrescriptiveEvent">
		<rdfs:label>prescriptive event</rdfs:label>
		<skos:definition>An event whereby a debt security comes to the end of its life and the debt is paid off (redeemed).</skos:definition>
	</owl:Class>
	
	<owl:Class
		rdf:about="&fibo-sec-dbt-dbt-cft;PrincipalOnly">
		<rdfs:subClassOf
			rdf:resource="&fibo-sec-dbt-dbt-cft;AmortizationType"/>
		<rdfs:label>principal only</rdfs:label>
	</owl:Class>
	
	<owl:Class
		rdf:about="&fibo-sec-dbt-dbt-cft;PrincipalPlusInterest">
		<rdfs:subClassOf
			rdf:resource="&fibo-sec-dbt-dbt-cft;AmortizationType"/>
		<rdfs:label>principal plus interest</rdfs:label>
	</owl:Class>
	
	<owl:Class
		rdf:about="&fibo-sec-dbt-dbt-cft;PutDate">
		<rdfs:subClassOf
			rdf:resource="&fibo-sec-sec-schx;ScheduledEventDate"/>
		<rdfs:label>put date</rdfs:label>
		<skos:definition>Date on which the instrument may be put.</skos:definition>
	</owl:Class>
	
	<owl:Class
		rdf:about="&fibo-sec-dbt-dbt-cft;PutOfIssue">
		<rdfs:subClassOf
			rdf:resource="&fibo-sec-dbt-dbt-cft;RedemptionEvent"/>
		<rdfs:subClassOf
			rdf:resource="&fibo-sec-sec-schx;ExplicitlyScheduledEvent"/>
		<rdfs:subClassOf>
			<owl:Restriction>
				<owl:onProperty
					rdf:resource="&fibo-sec-dbt-dbt-cft;occursOn.1"/>
				<owl:someValuesFrom
					rdf:resource="&fibo-sec-dbt-dbt-cft;PutDate"/>
			</owl:Restriction>
		</rdfs:subClassOf>
		<rdfs:label>put of issue</rdfs:label>
		<skos:definition>The putting i.e. the giving up of units of a Traded Security by Holders.</skos:definition>
	</owl:Class>
	
	<owl:Class
		rdf:about="&fibo-sec-dbt-dbt-cft;PutSchedule">
		<rdfs:subClassOf
			rdf:resource="&fibo-fnd-dt-fd;Schedule"/>
		<rdfs:label>put schedule</rdfs:label>
	</owl:Class>
	
	<owl:Class
		rdf:about="&fibo-sec-dbt-dbt-cft;PutScheduleListing">
		<rdfs:subClassOf
			rdf:resource="&fibo-fnd-dt-fd;AdHocSchedule"/>
		<rdfs:subClassOf
			rdf:resource="&fibo-sec-dbt-dbt-cft;PutSchedule"/>
		<rdfs:subClassOf>
			<owl:Restriction>
				<owl:onProperty
					rdf:resource="&fibo-sec-sec-schx;listsScheduledEvent"/>
				<owl:someValuesFrom
					rdf:resource="&fibo-sec-dbt-dbt-cft;PutOfIssue"/>
			</owl:Restriction>
		</rdfs:subClassOf>
		<rdfs:label>put schedule listing</rdfs:label>
		<skos:definition>Schedule of dates on which a Traded Security may be Put by the Holder.</skos:definition>
	</owl:Class>
	
	<owl:Class
		rdf:about="&fibo-sec-dbt-dbt-cft;PutTerms">
		<rdfs:subClassOf
			rdf:resource="&fibo-fnd-agr-ctr;ContractualCommitment"/>
		<rdfs:subClassOf>
			<owl:Restriction>
				<owl:onProperty
					rdf:resource="&fibo-sec-dbt-dbt-cft;includes"/>
				<owl:someValuesFrom
					rdf:resource="&fibo-sec-dbt-dbt-cft;PutSchedule"/>
			</owl:Restriction>
		</rdfs:subClassOf>
		<rdfs:subClassOf>
			<owl:Restriction>
				<owl:onProperty
					rdf:resource="&fibo-sec-dbt-dbt-cft;includesWindow.1"/>
				<owl:someValuesFrom
					rdf:resource="&fibo-sec-dbt-dbt-cft;PutWindow"/>
			</owl:Restriction>
		</rdfs:subClassOf>
		<rdfs:label>put terms</rdfs:label>
		<skos:definition>Contractual terms for a feature that provides the bond holder the contractual option to redeem the bond prior to the scheduled maturity date.</skos:definition>
		<skos:editorialNote>FIBIM has term &quot;Putable Date&quot; which (by implication, and comparing with definition for &quot;Next Call Date&quot;) is presumably a single calendar date in the future, at a given point in time. That does not cover the definition of formal terms defining when and how the issue may be put, which is what is modeled here.</skos:editorialNote>
	</owl:Class>
	
	<owl:Class
		rdf:about="&fibo-sec-dbt-dbt-cft;PutWindow">
		<rdfs:subClassOf
			rdf:resource="&fibo-fnd-tim-tim;DurationDescriptionInCalendarTemporalUnit"/>
		<rdfs:subClassOf>
			<owl:Restriction>
				<owl:onProperty
					rdf:resource="&fibo-sec-dbt-dbt-cft;hasPutCalendarType"/>
				<owl:someValuesFrom
					rdf:resource="&fibo-sec-dbt-dbt-cft;CalendarType"/>
			</owl:Restriction>
		</rdfs:subClassOf>
		<rdfs:label>put window</rdfs:label>
		<skos:definition>Window of number of days prior to a mandatory or optional redemption date that the issuer/agent must give notice to holders.</skos:definition>
	</owl:Class>
	
	<owl:Class
		rdf:about="&fibo-sec-dbt-dbt-cft;RedemptionEvent">
		<rdfs:subClassOf
			rdf:resource="&fibo-sec-dbt-dbt-cft;PrescriptiveEvent"/>
		<rdfs:label>redemption event</rdfs:label>
		<skos:definition>An event whereby a debt security comes to the end of its life and the debt is paid off (redeemed).</skos:definition>
	</owl:Class>
	
	<owl:Class
		rdf:about="&fibo-sec-dbt-dbt-cft;SecuritizedDebtInterest">
		<rdfs:subClassOf
			rdf:resource="https://spec.edmcouncil.org/fibo/FBC/DebtAndEquities/Debt/Interest"/>
		<rdfs:label>securitized debt interest</rdfs:label>
		<skos:definition>Interest on Debt which is the subject of a Financial Security.</skos:definition>
	</owl:Class>
	
	<owl:Class
		rdf:about="&fibo-sec-dbt-dbt-cft;TradableDebtSecurityRedemptionTermsSet">
		<rdfs:subClassOf
			rdf:resource="https://spec.edmcouncil.org/fibo/FBC/DebtAndEquities/Debt/PrincipalRepaymentTerms"/>
		<rdfs:subClassOf>
			<owl:Restriction>
				<owl:maxQualifiedCardinality
					rdf:datatype="&xsd;nonNegativeInteger">1</owl:maxQualifiedCardinality>
				<owl:onClass
					rdf:resource="&fibo-sec-dbt-dbt-cft;ExtendableMaturityRedemptionTermsSet"/>
				<owl:onProperty
					rdf:resource="&fibo-sec-dbt-dbt-cft;includesForExtendableMaturity"/>
			</owl:Restriction>
		</rdfs:subClassOf>
		<rdfs:label>tradable debt security redemption terms set</rdfs:label>
		<skos:definition>Terms for the redemption of the debt represented by a debt security.</skos:definition>
		<skos:editorialNote>Debt represented by a tradable debt security may be paid as a one off payment at maturity, by paying down principal amounts periodically, or by a call of the issue by the issuer. Debt that is defined by a convertible bond are redeemed by conversion into an equity security issued by the same company. More notes from the EDMC SME Review: Distinction between call and amortizing is whether you pay off everybody at the same time or via a lottery. SF can be either. either amortize the payment of a SF or pay it off by a lottery. The terms of the instrument determine that. Mandatory - all in the schedule. Mandatory to the bond issuer. Issuer has to pay off a certain amount at a certain time - this is in the Schedule. Callable - nothing mandatory.</skos:editorialNote>
	</owl:Class>
	
	<owl:ObjectProperty
		rdf:about="&fibo-sec-dbt-dbt-cft;amount">
		<rdfs:label>amount</rdfs:label>
		<rdfs:domain
			rdf:resource="&fibo-sec-dbt-dbt-cft;Margin"/>
		<rdfs:range
			rdf:resource="&fibo-fnd-utl-val;PercentageValue"/>
		<skos:definition>A fixed, constant amount which forms the Margin parameter, expressed as a percentage.</skos:definition>
	</owl:ObjectProperty>
	
	<owl:ObjectProperty
		rdf:about="&fibo-sec-dbt-dbt-cft;autoReinvestment">
		<rdfs:label>auto reinvestment</rdfs:label>
		<rdfs:domain
			rdf:resource="&fibo-sec-dbt-dbt-cft;DebtSecurityInterestPaymentTerms"/>
		<rdfs:range
			rdf:resource="&fibo-fnd-utl-val;TrueFalseValue"/>
		<skos:definition>Whether the security provides for mandatorily &amp; automatically re-investing the interest from that security towards buying more of the same security.</skos:definition>
	</owl:ObjectProperty>
	
	<owl:ObjectProperty
		rdf:about="&fibo-sec-dbt-dbt-cft;callableByDebtor">
		<rdfs:label>callable by debtor</rdfs:label>
		<rdfs:domain
			rdf:resource="&fibo-sec-dbt-dbt-cft;DebtCallTerms"/>
		<rdfs:range
			rdf:resource="&fibo-fnd-utl-val;TrueFalseValue"/>
	</owl:ObjectProperty>
	
	<owl:ObjectProperty
		rdf:about="&fibo-sec-dbt-dbt-cft;compoundingFrequency">
		<rdfs:label>compounding frequency</rdfs:label>
		<rdfs:domain
			rdf:resource="&fibo-sec-dbt-dbt-cft;DebtSecurityInterestPaymentTerms"/>
		<rdfs:range
			rdf:resource="&fibo-fnd-tim-tim;Frequency"/>
		<skos:definition>The frequency at which the interest is compounded. This is established at the initial stages of securing the instrument. Generally, interest tends to be calculated on an annual basis although other terms may be established at the time of the loan.</skos:definition>
	</owl:ObjectProperty>
	
	<owl:ObjectProperty
		rdf:about="&fibo-sec-dbt-dbt-cft;datedDate">
		<rdfs:label>dated date</rdfs:label>
		<terms:description>the date on which an interest paying debt instrument begins to accrue interest</terms:description>
		<rdfs:domain
			rdf:resource="&fibo-sec-dbt-dbt-cft;DebtSecurityInterestPaymentTerms"/>
		<rdfs:range
			rdf:resource="&fibo-fnd-tim-tim;Date"/>
	</owl:ObjectProperty>
	
	<owl:ObjectProperty
		rdf:about="&fibo-sec-dbt-dbt-cft;daysToCallNotification">
		<rdfs:label>days to call notification</rdfs:label>
		<rdfs:domain
			rdf:resource="&fibo-sec-dbt-dbt-cft;NotificationFeature"/>
		<rdfs:range
			rdf:resource="&fibo-fnd-utl-val;IntegerValue"/>
		<skos:definition>Number of days prior to a call date that the issuer/agent must give notice to holders.</skos:definition>
	</owl:ObjectProperty>
	
	<owl:ObjectProperty
		rdf:about="&fibo-sec-dbt-dbt-cft;daysToPut">
		<rdfs:label>days to put</rdfs:label>
		<rdfs:domain
			rdf:resource="&fibo-sec-dbt-dbt-cft;PutTerms"/>
		<rdfs:range
			rdf:resource="&fibo-fnd-utl-val;IntegerValue"/>
		<skos:definition>Number of days prior to a mandatory or optional redemption date that the issuer/agent must give notice to holders.</skos:definition>
	</owl:ObjectProperty>
	
	<owl:ObjectProperty
		rdf:about="&fibo-sec-dbt-dbt-cft;daysToPutNotification">
		<rdfs:label>days to put notification</rdfs:label>
		<rdfs:domain
			rdf:resource="&fibo-sec-dbt-dbt-cft;PutWindow"/>
		<rdfs:range
			rdf:resource="&fibo-fnd-utl-val;IntegerValue"/>
		<skos:definition>Number of days prior to a mandatory or optional redemption date that the issuer/agent must give notice to holders. This term replaces the Multipler term in the Duratiojn Description.</skos:definition>
	</owl:ObjectProperty>
	
	<owl:ObjectProperty
		rdf:about="&fibo-sec-dbt-dbt-cft;estateOrDeathPut">
		<rdfs:label>estate or death put</rdfs:label>
		<rdfs:domain
			rdf:resource="&fibo-sec-dbt-dbt-cft;PutTerms"/>
		<rdfs:range
			rdf:resource="&fibo-fnd-utl-val;TrueFalseValue"/>
		<skos:definition>Specifies that a security is subject to be Redeemed upon the passing of the holder.</skos:definition>
	</owl:ObjectProperty>
	
	<owl:ObjectProperty
		rdf:about="&fibo-sec-dbt-dbt-cft;expression">
		<rdfs:label>expression</rdfs:label>
		<rdfs:domain
			rdf:resource="&fibo-sec-dbt-dbt-cft;InterestCalculationExpression"/>
		<rdfs:range
			rdf:resource="&fibo-fnd-utl-val;TextValue"/>
		<skos:definition>Textual expression of the entire right hand side of the Formula. Note that this is additional to the modelling of the separate Arguments that make up the formula.</skos:definition>
	</owl:ObjectProperty>
	
	<owl:ObjectProperty
		rdf:about="&fibo-sec-dbt-dbt-cft;extendableByHolder">
		<rdfs:label>extendable by holder</rdfs:label>
		<rdfs:domain
			rdf:resource="&fibo-sec-dbt-dbt-cft;TradableDebtSecurityRedemptionTermsSet"/>
		<rdfs:range
			rdf:resource="&fibo-fnd-utl-val;TrueFalseValue"/>
		<skos:definition>Indicates whether the expiration date or maturity date can be extended by the holder, i.e. repayment may be extended or maturity changed.</skos:definition>
	</owl:ObjectProperty>
	
	<owl:ObjectProperty
		rdf:about="&fibo-sec-dbt-dbt-cft;extendableByIssuer">
		<rdfs:label>extendable by issuer</rdfs:label>
		<rdfs:domain
			rdf:resource="&fibo-sec-dbt-dbt-cft;TradableDebtSecurityRedemptionTermsSet"/>
		<rdfs:range
			rdf:resource="&fibo-fnd-utl-val;TrueFalseValue"/>
		<skos:definition>Whether the issuer has the option to extend the debt rather than refinancing. If not, the issuer may only refinance the debt by calling the issue and creating a new issue.</skos:definition>
	</owl:ObjectProperty>
	
	<owl:ObjectProperty
		rdf:about="&fibo-sec-dbt-dbt-cft;extendableDate">
		<rdfs:label>extendable date</rdfs:label>
		<rdfs:domain
			rdf:resource="&fibo-sec-dbt-dbt-cft;ExtendableMaturityRedemptionTermsSet"/>
		<rdfs:range
			rdf:resource="&fibo-fnd-tim-tim;DeterminedDate"/>
		<skos:definition>Date to which the Maturity Date may be extended. This date is determined at the set-up of the bond. Note this date is adjustable according to various applicable parameters or terms. May have a rolling extendable maturity date. The bond holder may choose to extend. Usually a 13 month rolling extendable maturity.</skos:definition>
	</owl:ObjectProperty>
	
	<owl:ObjectProperty
		rdf:about="&fibo-sec-dbt-dbt-cft;extendablePeriod">
		<rdfs:label>extendable period</rdfs:label>
		<rdfs:domain
			rdf:resource="&fibo-sec-dbt-dbt-cft;ExtendableMaturityRedemptionTermsSet"/>
		<rdfs:range
			rdf:resource="&fibo-fnd-tim-tim;DatePeriod"/>
		<skos:definition>Period during which the Maturity Date may be extended.</skos:definition>
	</owl:ObjectProperty>
	
	<owl:ObjectProperty
		rdf:about="&fibo-sec-dbt-dbt-cft;extraordinaryCallProvision">
		<rdfs:label>extraordinary call provision</rdfs:label>
		<rdfs:domain
			rdf:resource="&fibo-sec-dbt-dbt-cft;DebtCallTerms"/>
		<rdfs:range
			rdf:resource="&fibo-fnd-utl-val;TrueFalseValue"/>
		<skos:definition>Indicates the existence of an Extraordinary Call provision in the bond call terms.</skos:definition>
	</owl:ObjectProperty>
	
	<owl:ObjectProperty
		rdf:about="&fibo-sec-dbt-dbt-cft;firstInterestAccrualDate">
		<rdfs:label>first interest accrual date</rdfs:label>
		<rdfs:domain
			rdf:resource="&fibo-sec-dbt-dbt-cft;DebtSecurityInterestPaymentTerms"/>
		<rdfs:range
			rdf:resource="&fibo-fnd-dt-fd;Date"/>
		<skos:definition>Date from which the security begins to accrue interest.</skos:definition>
	</owl:ObjectProperty>
	
	<owl:ObjectProperty
		rdf:about="&fibo-sec-dbt-dbt-cft;firstInterestPaymentDate">
		<rdfs:label>first interest payment date</rdfs:label>
		<rdfs:domain
			rdf:resource="&fibo-sec-dbt-dbt-cft;DebtSecurityInterestPaymentTerms"/>
		<rdfs:range
			rdf:resource="&fibo-fnd-dt-fd;Date"/>
		<skos:definition>The day on which the first interest payment is due to the holders of the security.</skos:definition>
	</owl:ObjectProperty>
	
	<owl:ObjectProperty
		rdf:about="&fibo-sec-dbt-dbt-cft;firstParCallDate">
		<rdfs:label>first par call date</rdfs:label>
		<rdfs:domain
			rdf:resource="&fibo-sec-dbt-dbt-cft;DebtCallTerms"/>
		<rdfs:range
			rdf:resource="&fibo-fnd-dt-fd;Date"/>
		<skos:definition>The first date on which bonds may be called at Par for redemption.</skos:definition>
	</owl:ObjectProperty>
	
	<owl:ObjectProperty
		rdf:about="&fibo-sec-dbt-dbt-cft;firstParCallPrice">
		<rdfs:label>first par call price</rdfs:label>
		<rdfs:domain
			rdf:resource="&fibo-sec-dbt-dbt-cft;DebtCallTerms"/>
		<rdfs:range
			rdf:resource="&fibo-fnd-utl-val;PercentageValue"/>
		<skos:definition>The price of the bonds on the first Par part call.</skos:definition>
	</owl:ObjectProperty>
	
	<owl:ObjectProperty
		rdf:about="&fibo-sec-dbt-dbt-cft;firstPremiumCallDate">
		<rdfs:label>first premium call date</rdfs:label>
		<rdfs:domain
			rdf:resource="&fibo-sec-dbt-dbt-cft;DebtCallTerms"/>
		<rdfs:range
			rdf:resource="&fibo-fnd-dt-fd;Date"/>
		<skos:definition>The first date on which bonds may be called for redemption at a price above par.</skos:definition>
	</owl:ObjectProperty>
	
	<owl:ObjectProperty
		rdf:about="&fibo-sec-dbt-dbt-cft;firstPremiumCallPrice">
		<rdfs:label>first premium call price</rdfs:label>
		<rdfs:domain
			rdf:resource="&fibo-sec-dbt-dbt-cft;DebtCallTerms"/>
		<rdfs:range
			rdf:resource="&fibo-fnd-utl-val;PercentageValue"/>
		<skos:definition>The price of the bonds on the first part call at a price above par.</skos:definition>
	</owl:ObjectProperty>
	
	<owl:ObjectProperty
		rdf:about="&fibo-sec-dbt-dbt-cft;hasAccrualBasis">
		<rdfs:subPropertyOf
			rdf:resource="&fibo-fnd-agr-ctr;isQualifiedBy"/>
		<rdfs:label>has accrual basis</rdfs:label>
		<rdfs:domain
			rdf:resource="&fibo-sec-dbt-dbt-cft;DebtSecurityInterestPaymentTerms"/>
		<rdfs:range
			rdf:resource="&fibo-sec-dbt-dbt-dbt;DayCountBasis"/>
	</owl:ObjectProperty>
	
	<owl:ObjectProperty
		rdf:about="&fibo-sec-dbt-dbt-cft;hasBaseParameter">
		<rdfs:subPropertyOf
			rdf:resource="&fibo-fnd-math-math;hasArgument"/>
		<rdfs:label>has base parameter</rdfs:label>
		<rdfs:domain
			rdf:resource="&fibo-sec-dbt-dbt-cft;InterestCalculationExpression"/>
		<rdfs:range
			rdf:resource="&fibo-sec-dbt-dbt-cft;Base"/>
	</owl:ObjectProperty>
	
	<owl:ObjectProperty
		rdf:about="&fibo-sec-dbt-dbt-cft;hasFormula">
		<rdfs:subPropertyOf
			rdf:resource="&fibo-fnd-agr-ctr;isQualifiedBy"/>
		<rdfs:label>has formula</rdfs:label>
		<rdfs:domain
			rdf:resource="&fibo-sec-dbt-dbt-cft;DebtSecurityInterestPaymentTerms"/>
		<rdfs:range
			rdf:resource="&fibo-sec-dbt-dbt-cft;InterestCalculationFormula"/>
	</owl:ObjectProperty>
	
	<owl:ObjectProperty
		rdf:about="&fibo-sec-dbt-dbt-cft;hasInterestTerms">
		<rdfs:label>has interest terms</rdfs:label>
	</owl:ObjectProperty>
	
	<owl:ObjectProperty
		rdf:about="&fibo-sec-dbt-dbt-cft;hasMarginParameter">
		<rdfs:subPropertyOf
			rdf:resource="&fibo-fnd-math-math;hasArgument"/>
		<rdfs:label>has margin parameter</rdfs:label>
		<rdfs:domain
			rdf:resource="&fibo-sec-dbt-dbt-cft;InterestCalculationExpression"/>
		<rdfs:range
			rdf:resource="&fibo-sec-dbt-dbt-cft;Margin"/>
	</owl:ObjectProperty>
	
	<owl:ObjectProperty
		rdf:about="&fibo-sec-dbt-dbt-cft;hasNotificationFeature">
		<rdfs:label>has notification feature</rdfs:label>
		<rdfs:domain
			rdf:resource="&fibo-sec-dbt-dbt-cft;DebtCallTerms"/>
		<rdfs:range
			rdf:resource="&fibo-sec-dbt-dbt-cft;NotificationFeature"/>
	</owl:ObjectProperty>
	
	<owl:ObjectProperty
		rdf:about="&fibo-sec-dbt-dbt-cft;hasPerpetualCall">
		<rdfs:label>has perpetual call</rdfs:label>
		<terms:description>the asset has a perpetual call schedule</terms:description>
		<rdfs:domain
			rdf:resource="&fibo-sec-dbt-dbt-cft;DebtCallTerms"/>
		<rdfs:range
			rdf:resource="&fibo-fnd-utl-val;TrueFalseValue"/>
	</owl:ObjectProperty>
	
	<owl:ObjectProperty
		rdf:about="&fibo-sec-dbt-dbt-cft;hasPrincipalAmortizationType">
		<rdfs:label>has principal amortization type</rdfs:label>
		<rdfs:domain
			rdf:resource="https://spec.edmcouncil.org/fibo/FBC/DebtAndEquities/Debt/PrincipalRepaymentTerms"/>
		<rdfs:range
			rdf:resource="&fibo-sec-dbt-dbt-cft;AmortizationType"/>
		<skos:definition>The type of principal payments applicable to this security.</skos:definition>
	</owl:ObjectProperty>
	
	<owl:ObjectProperty
		rdf:about="&fibo-sec-dbt-dbt-cft;hasPutCalendarType">
		<rdfs:subPropertyOf
			rdf:resource="&fibo-fnd-tim-tim;hasCalendarDenomination"/>
		<rdfs:label>has put calendar type</rdfs:label>
		<rdfs:domain
			rdf:resource="&fibo-sec-dbt-dbt-cft;PutWindow"/>
		<rdfs:range
			rdf:resource="&fibo-sec-dbt-dbt-cft;CalendarType"/>
	</owl:ObjectProperty>
	
	<owl:ObjectProperty
		rdf:about="&fibo-sec-dbt-dbt-cft;hasRedemptionTerms">
		<rdfs:label>has redemption terms</rdfs:label>
	</owl:ObjectProperty>
	
	<owl:ObjectProperty
		rdf:about="&fibo-sec-dbt-dbt-cft;includes">
		<rdfs:label>includes</rdfs:label>
		<rdfs:domain
			rdf:resource="&fibo-sec-dbt-dbt-cft;PutTerms"/>
		<rdfs:range
			rdf:resource="&fibo-sec-dbt-dbt-cft;PutSchedule"/>
	</owl:ObjectProperty>
	
	<owl:ObjectProperty
		rdf:about="&fibo-sec-dbt-dbt-cft;includesForExtendableMaturity">
		<rdfs:label>includes for extendable maturity</rdfs:label>
		<rdfs:domain
			rdf:resource="&fibo-sec-dbt-dbt-cft;TradableDebtSecurityRedemptionTermsSet"/>
		<rdfs:range
			rdf:resource="&fibo-sec-dbt-dbt-cft;ExtendableMaturityRedemptionTermsSet"/>
		<skos:definition>In the case of terms where extendable maturity is yes, terms are included regarding the extension of the maturity on the security.</skos:definition>
	</owl:ObjectProperty>
	
	<owl:ObjectProperty
		rdf:about="&fibo-sec-dbt-dbt-cft;includesWindow.1">
		<rdfs:label>includes window</rdfs:label>
		<rdfs:domain
			rdf:resource="&fibo-sec-dbt-dbt-cft;PutTerms"/>
		<rdfs:range
			rdf:resource="&fibo-sec-dbt-dbt-cft;PutWindow"/>
	</owl:ObjectProperty>
	
	<owl:ObjectProperty
		rdf:about="&fibo-sec-dbt-dbt-cft;interestPaymentDayAndMonth">
		<rdfs:label>interest payment day and month</rdfs:label>
		<rdfs:domain
			rdf:resource="&fibo-sec-dbt-dbt-cft;DebtSecurityInterestPaymentTerms"/>
		<rdfs:range
			rdf:resource="&fibo-fnd-utl-val;DayMonthValue"/>
		<skos:definition>The regular dates of interest payment in any given year during the life of the debt instrument.</skos:definition>
	</owl:ObjectProperty>
	
	<owl:ObjectProperty
		rdf:about="&fibo-sec-dbt-dbt-cft;interestPaymentFrequency">
		<rdfs:label>interest payment frequency</rdfs:label>
		<rdfs:domain
			rdf:resource="&fibo-sec-dbt-dbt-cft;DebtSecurityInterestPaymentTerms"/>
		<rdfs:range
			rdf:resource="&fibo-fnd-tim-tim;Frequency"/>
		<skos:definition>Frequency of payment of Interest on the debt.</skos:definition>
	</owl:ObjectProperty>
	
	<owl:ObjectProperty
		rdf:about="&fibo-sec-dbt-dbt-cft;interestRate">
		<rdfs:label>interest rate</rdfs:label>
		<rdfs:domain
			rdf:resource="&fibo-sec-dbt-dbt-cft;NonTradableDebtInterestTerms"/>
		<rdfs:range
			rdf:resource="&fibo-fnd-utl-val;PercentageValue"/>
		<skos:definition>The annual percentage rate of interest that must be paid on the debt.</skos:definition>
	</owl:ObjectProperty>
	
	<owl:ObjectProperty
		rdf:about="&fibo-sec-dbt-dbt-cft;isLegallyDefeased">
		<rdfs:label>is legally defeased</rdfs:label>
		<terms:description>whether the maturity is legally defeased</terms:description>
		<rdfs:domain
			rdf:resource="&fibo-sec-dbt-dbt-cft;TradableDebtSecurityRedemptionTermsSet"/>
		<rdfs:range
			rdf:resource="&fibo-fnd-utl-val;TrueFalseValue"/>
	</owl:ObjectProperty>
	
	<owl:ObjectProperty
		rdf:about="&fibo-sec-dbt-dbt-cft;lastInterestPaymentDate">
		<rdfs:label>last interest payment date</rdfs:label>
		<rdfs:domain
			rdf:resource="&fibo-sec-dbt-dbt-cft;DebtSecurityInterestPaymentTerms"/>
		<rdfs:range
			rdf:resource="&fibo-fnd-dt-fd;Date"/>
		<skos:definition>The day on which the final interest payment is due to the holders of the security prior to maturity. This is only needed if the last coupon is of an odd length.</skos:definition>
	</owl:ObjectProperty>
	
	<owl:ObjectProperty
		rdf:about="&fibo-sec-dbt-dbt-cft;legalFinalMaturityDate">
		<rdfs:label>legal final maturity date</rdfs:label>
		<rdfs:domain
			rdf:resource="&fibo-sec-dbt-dbt-cft;TradableDebtSecurityRedemptionTermsSet"/>
		<rdfs:range
			rdf:resource="&fibo-fnd-dt-fd;Date"/>
		<skos:definition>the date on which the principal must be paid to investors</skos:definition>
		<fibo-fnd-utl-av:explanatoryNote>The Legal Maturity Date is later than the expected maturity date and is the date on which the principal must be paid to investors. Also called final maturity date. It is also the termination or due date on which an installment loan must be paid in full.</fibo-fnd-utl-av:explanatoryNote>
	</owl:ObjectProperty>
	
	<owl:ObjectProperty
		rdf:about="&fibo-sec-dbt-dbt-cft;makeWholeCallProvision">
		<rdfs:label>make whole call provision</rdfs:label>
		<rdfs:domain
			rdf:resource="&fibo-sec-dbt-dbt-cft;DebtCallTerms"/>
		<rdfs:range
			rdf:resource="&fibo-fnd-utl-val;TrueFalseValue"/>
		<skos:definition>A provision on the bond allowing the borrower to pay off remaining debt early.</skos:definition>
		<skos:definition>A type of call provision allowing the issuer to pay off debt early that is designed to protect the investor from losses as a result of the earlier call. In order to exercise the call, the issuer must make a lump sum payment derived from a formula based on the net present value of future interest payments that will not be paid as a result of the call.</skos:definition>
		<fibo-fnd-utl-av:definitionOrigin>http://www.msrb.org/Glossary/Definition/MAKE-WHOLE-CALL.aspx</fibo-fnd-utl-av:definitionOrigin>
		<fibo-fnd-utl-av:explanatoryNote>Because the cost can often be significant, such provisions are rarely used.</fibo-fnd-utl-av:explanatoryNote>
	</owl:ObjectProperty>
	
	<owl:ObjectProperty
		rdf:about="&fibo-sec-dbt-dbt-cft;mandatoryPut">
		<rdfs:label>mandatory put</rdfs:label>
		<rdfs:domain
			rdf:resource="&fibo-sec-dbt-dbt-cft;PutTerms"/>
		<rdfs:range
			rdf:resource="&fibo-fnd-utl-val;TrueFalseValue"/>
		<skos:definition>Whether the redemption prior to maturity date feature is Mandatory to the bond holder. If No, then this is optional.</skos:definition>
	</owl:ObjectProperty>
	
	<owl:ObjectProperty
		rdf:about="&fibo-sec-dbt-dbt-cft;mandatorySinkingFund">
		<rdfs:label>mandatory sinking fund</rdfs:label>
		<rdfs:domain
			rdf:resource="&fibo-sec-dbt-dbt-cft;DebtCallTerms"/>
		<rdfs:range
			rdf:resource="&fibo-fnd-utl-val;TrueFalseValue"/>
		<skos:definition>Whether there is a Mandatory Sinking fund feature.</skos:definition>
	</owl:ObjectProperty>
	
	<owl:ObjectProperty
		rdf:about="&fibo-sec-dbt-dbt-cft;notification">
		<rdfs:label>notification</rdfs:label>
		<rdfs:domain
			rdf:resource="&fibo-sec-dbt-dbt-cft;NotificationFeature"/>
		<rdfs:range
			rdf:resource="&fibo-fnd-utl-val;TrueFalseValue"/>
		<skos:definition>Whether Call Schedule includes notification.</skos:definition>
	</owl:ObjectProperty>
	
	<owl:ObjectProperty
		rdf:about="&fibo-sec-dbt-dbt-cft;occursOn.1">
		<rdfs:subPropertyOf
			rdf:resource="&fibo-sec-sec-schx;hasEventDate"/>
		<rdfs:label>occurs on</rdfs:label>
		<rdfs:domain
			rdf:resource="&fibo-sec-dbt-dbt-cft;PutOfIssue"/>
		<rdfs:range
			rdf:resource="&fibo-sec-dbt-dbt-cft;PutDate"/>
	</owl:ObjectProperty>
	
	<owl:ObjectProperty
		rdf:about="&fibo-sec-dbt-dbt-cft;payInKind">
		<rdfs:label>pay in kind</rdfs:label>
		<rdfs:domain
			rdf:resource="&fibo-sec-dbt-dbt-cft;DebtSecurityInterestPaymentTerms"/>
		<rdfs:range
			rdf:resource="&fibo-fnd-utl-val;TrueFalseValue"/>
		<skos:definition>The issuer will pay additional security as part of interest disbursement. Review: This needs to be replaced wit a sub class of Interst Payment in which the additional security is specified.</skos:definition>
	</owl:ObjectProperty>
	
	<owl:ObjectProperty
		rdf:about="&fibo-sec-dbt-dbt-cft;paymentInKind">
		<rdfs:label>payment in kind</rdfs:label>
		<rdfs:domain
			rdf:resource="&fibo-sec-dbt-dbt-cft;TradableDebtSecurityRedemptionTermsSet"/>
		<rdfs:range
			rdf:resource="&fibo-fnd-utl-val;TrueFalseValue"/>
		<skos:definition>Whether the Principal may be repaid in kind rather than in cash.</skos:definition>
	</owl:ObjectProperty>
	
	<owl:ObjectProperty
		rdf:about="&fibo-sec-dbt-dbt-cft;perpetualMaturity">
		<rdfs:label>perpetual maturity</rdfs:label>
		<rdfs:domain
			rdf:resource="&fibo-sec-dbt-dbt-cft;TradableDebtSecurityRedemptionTermsSet"/>
		<rdfs:range
			rdf:resource="&fibo-fnd-utl-val;TrueFalseValue"/>
		<skos:definition>Whether the debt security has perpetual maturity, i.e. there is no Maturity Date and the security remains in issue indefinitely or until recalled.</skos:definition>
	</owl:ObjectProperty>
	
	<owl:ObjectProperty
		rdf:about="&fibo-sec-dbt-dbt-cft;proRated">
		<rdfs:label>pro rated</rdfs:label>
		<rdfs:domain
			rdf:resource="&fibo-sec-dbt-dbt-cft;DebtSecurityInterestPaymentTerms"/>
		<rdfs:range
			rdf:resource="&fibo-fnd-utl-val;TrueFalseValue"/>
		<skos:definition>Whether the coupon is pro rated to the actual number of days in the payment period versus the number of payment periods.</skos:definition>
	</owl:ObjectProperty>
	
	<owl:ObjectProperty
		rdf:about="&fibo-sec-dbt-dbt-cft;putDate">
		<rdfs:label>put date</rdfs:label>
		<rdfs:domain
			rdf:resource="&fibo-sec-dbt-dbt-cft;PutTerms"/>
		<rdfs:range
			rdf:resource="&fibo-fnd-dt-fd;Date"/>
		<skos:definition>Date on which securities are subject to Optional or Mandatory Redemption by the bond holder.</skos:definition>
	</owl:ObjectProperty>
	
	<owl:ObjectProperty
		rdf:about="&fibo-sec-dbt-dbt-cft;putFrequency">
		<rdfs:label>put frequency</rdfs:label>
		<rdfs:domain
			rdf:resource="&fibo-sec-dbt-dbt-cft;PutTerms"/>
		<rdfs:range
			rdf:resource="&fibo-fnd-tim-tim;Frequency"/>
		<skos:definition>Frequency of Tender or Put period.</skos:definition>
	</owl:ObjectProperty>
	
	<owl:ObjectProperty
		rdf:about="&fibo-sec-dbt-dbt-cft;rightToRetain">
		<rdfs:label>right to retain</rdfs:label>
		<rdfs:domain
			rdf:resource="&fibo-sec-dbt-dbt-cft;PutTerms"/>
		<rdfs:range
			rdf:resource="&fibo-fnd-utl-val;TrueFalseValue"/>
		<skos:definition>Whether the holder has an option to retain the security in the event of an issuer exercising the put option.</skos:definition>
	</owl:ObjectProperty>
	
	<owl:ObjectProperty
		rdf:about="&fibo-sec-dbt-dbt-cft;roundingDecimalPlaces">
		<rdfs:label>rounding decimal places</rdfs:label>
		<rdfs:domain
			rdf:resource="&fibo-sec-dbt-dbt-cft;Base"/>
		<rdfs:range
			rdf:resource="&fibo-fnd-utl-val;IntegerValue"/>
		<skos:definition>Number of decimal places to round to.</skos:definition>
	</owl:ObjectProperty>
	
	<owl:ObjectProperty
		rdf:about="&fibo-sec-dbt-dbt-cft;scheduledMaturityDate">
		<rdfs:label>scheduled maturity date</rdfs:label>
		<rdfs:domain
			rdf:resource="&fibo-sec-dbt-dbt-cft;TradableDebtSecurityRedemptionTermsSet"/>
		<rdfs:range
			rdf:resource="&fibo-fnd-dt-fd;Date"/>
		<skos:definition>Originally specified date on which an interest bearing security becomes due and assets are to be repaid, as stated in the security&apos;s offering documents. This is the date on which the principal amount of a debt instrument becomes due and is repaid to the investor and interest payments stop.</skos:definition>
	</owl:ObjectProperty>
	
	<owl:ObjectProperty
		rdf:about="&fibo-sec-dbt-dbt-cft;subjectIs">
		<rdfs:label>subject is</rdfs:label>
		<rdfs:domain
			rdf:resource="&fibo-sec-dbt-dbt-cft;InterestCalculationSubject"/>
		<rdfs:range
			rdf:resource="&fibo-sec-dbt-dbt-cft;SecuritizedDebtInterest"/>
	</owl:ObjectProperty>
	
	<owl:ObjectProperty
		rdf:about="&fibo-sec-dbt-dbt-cft;truncatingDecimalPlaces">
		<rdfs:label>truncating decimal places</rdfs:label>
		<rdfs:domain
			rdf:resource="&fibo-sec-dbt-dbt-cft;Base"/>
		<rdfs:range
			rdf:resource="&fibo-fnd-utl-val;IntegerValue"/>
		<skos:definition>Number of decimal places. Note this is either/or with the Rounding number of decimal places.</skos:definition>
	</owl:ObjectProperty>

</rdf:RDF>