<?xml version="1.0" encoding="UTF-8"?>
<!DOCTYPE rdf:RDF [
	<!ENTITY fibo-be-ge-ge "https://spec.edmcouncil.org/fibo/BE/GovernmentEntities/GovernmentEntities/">
	<!ENTITY fibo-be-le-fbo "https://spec.edmcouncil.org/fibo/BE/LegalEntities/FormalBusinessOrganizations/">
	<!ENTITY fibo-fnd-inf-doc "https://spec.edmcouncil.org/fibo/FND/Information/Documentation/">
	<!ENTITY fibo-fnd-inf-inf "https://spec.edmcouncil.org/fibo/FND/Information/InfoCore/">
	<!ENTITY fibo-fnd-plcx-re "https://spec.edmcouncil.org/fibo/FND/PlacesExt/RealEstate/">
	<!ENTITY fibo-fnd-pty-pty "https://spec.edmcouncil.org/fibo/FND/Parties/Parties/">
	<!ENTITY fibo-fnd-pty-rl "https://spec.edmcouncil.org/fibo/FND/Parties/Roles/">
	<!ENTITY fibo-fnd-rel-rel "https://spec.edmcouncil.org/fibo/FND/Relations/Relations/">
	<!ENTITY fibo-fnd-utl-av "https://spec.edmcouncil.org/fibo/FND/Utilities/AnnotationVocabulary/">
	<!ENTITY fibo-fnd-utl-val "https://spec.edmcouncil.org/fibo/FND/Utilities/Values/">
	<!ENTITY fibo-sec-dbt-dbt-gty "https://spec.edmcouncil.org/fibo/SEC/Debt/DebtFoundations/DebtInstrumentGuaranties/">
	<!ENTITY fibo-sec-dbt-dbt-gtyx "https://spec.edmcouncil.org/fibo/SEC/Debt/DebtFoundations/GuarantyExt/">
	<!ENTITY owl "http://www.w3.org/2002/07/owl#">
	<!ENTITY rdf "http://www.w3.org/1999/02/22-rdf-syntax-ns#">
	<!ENTITY rdfs "http://www.w3.org/2000/01/rdf-schema#">
	<!ENTITY skos "http://www.w3.org/2004/02/skos/core#">
	<!ENTITY xsd "http://www.w3.org/2001/XMLSchema#">
]>
<rdf:RDF xml:base="https://spec.edmcouncil.org/fibo/SEC/Debt/DebtFoundations/DebtInstrumentGuaranties/"
	xmlns:fibo-be-ge-ge="https://spec.edmcouncil.org/fibo/BE/GovernmentEntities/GovernmentEntities/"
	xmlns:fibo-be-le-fbo="https://spec.edmcouncil.org/fibo/BE/LegalEntities/FormalBusinessOrganizations/"
	xmlns:fibo-fnd-inf-doc="https://spec.edmcouncil.org/fibo/FND/Information/Documentation/"
	xmlns:fibo-fnd-inf-inf="https://spec.edmcouncil.org/fibo/FND/Information/InfoCore/"
	xmlns:fibo-fnd-plcx-re="https://spec.edmcouncil.org/fibo/FND/PlacesExt/RealEstate/"
	xmlns:fibo-fnd-pty-pty="https://spec.edmcouncil.org/fibo/FND/Parties/Parties/"
	xmlns:fibo-fnd-pty-rl="https://spec.edmcouncil.org/fibo/FND/Parties/Roles/"
	xmlns:fibo-fnd-rel-rel="https://spec.edmcouncil.org/fibo/FND/Relations/Relations/"
	xmlns:fibo-fnd-utl-av="https://spec.edmcouncil.org/fibo/FND/Utilities/AnnotationVocabulary/"
	xmlns:fibo-fnd-utl-val="https://spec.edmcouncil.org/fibo/FND/Utilities/Values/"
	xmlns:fibo-sec-dbt-dbt-gty="https://spec.edmcouncil.org/fibo/SEC/Debt/DebtFoundations/DebtInstrumentGuaranties/"
	xmlns:fibo-sec-dbt-dbt-gtyx="https://spec.edmcouncil.org/fibo/SEC/Debt/DebtFoundations/GuarantyExt/"
	xmlns:owl="http://www.w3.org/2002/07/owl#"
	xmlns:rdf="http://www.w3.org/1999/02/22-rdf-syntax-ns#"
	xmlns:rdfs="http://www.w3.org/2000/01/rdf-schema#"
	xmlns:skos="http://www.w3.org/2004/02/skos/core#"
	xmlns:xsd="http://www.w3.org/2001/XMLSchema#">
	
	<owl:Ontology rdf:about="https://spec.edmcouncil.org/fibo/SEC/Debt/DebtFoundations/DebtInstrumentGuaranties/">
		<rdfs:label xml:lang="en">DebtInstrumentGuaranties</rdfs:label>
		<owl:imports rdf:resource="http://www.w3.org/2000/01/rdf-schema"/>
		<owl:imports rdf:resource="http://www.w3.org/2004/02/skos/core"/>
		<owl:imports rdf:resource="https://spec.edmcouncil.org/fibo/BE/GovernmentEntities/GovernmentEntities/"/>
		<owl:imports rdf:resource="https://spec.edmcouncil.org/fibo/BE/LegalEntities/FormalBusinessOrganizations/"/>
		<owl:imports rdf:resource="https://spec.edmcouncil.org/fibo/FBC/DebtAndEquities/Debt/"/>
		<owl:imports rdf:resource="https://spec.edmcouncil.org/fibo/FBC/DebtAndEquities/Guaranty/"/>
		<owl:imports rdf:resource="https://spec.edmcouncil.org/fibo/FND/Information/Documentation/"/>
		<owl:imports rdf:resource="https://spec.edmcouncil.org/fibo/FND/Information/InfoCore/"/>
		<owl:imports rdf:resource="https://spec.edmcouncil.org/fibo/FND/Parties/Parties/"/>
		<owl:imports rdf:resource="https://spec.edmcouncil.org/fibo/FND/Parties/Roles/"/>
		<owl:imports rdf:resource="https://spec.edmcouncil.org/fibo/FND/PlacesExt/RealEstate/"/>
		<owl:imports rdf:resource="https://spec.edmcouncil.org/fibo/FND/Relations/Relations/"/>
		<owl:imports rdf:resource="https://spec.edmcouncil.org/fibo/FND/Utilities/AnnotationVocabulary/"/>
		<owl:imports rdf:resource="https://spec.edmcouncil.org/fibo/FND/Utilities/Values/"/>
		<owl:imports rdf:resource="https://spec.edmcouncil.org/fibo/SEC/Debt/DebtFoundations/GuarantyExt/"/>
	</owl:Ontology>
	
	<owl:Class rdf:about="&fibo-sec-dbt-dbt-gty;BondInsurance">
		<rdfs:subClassOf rdf:resource="&fibo-sec-dbt-dbt-gty;InsuranceBackedGuaranty"/>
		<rdfs:label xml:lang="en">bond insurance</rdfs:label>
		<skos:definition xml:lang="en">Insurance on bond.</skos:definition>
		<skos:editorialNote xml:lang="en">From April 21 Review: For cash CDOs: External e.g. Bond insurance that is bought from a 3rd party. NB Does not apply to synthetics. Also CDOs may have internal crefit enhancement instead. See main diagram note on this.</skos:editorialNote>
	</owl:Class>
	
	<owl:Class rdf:about="&fibo-sec-dbt-dbt-gty;CollateralizedGuaranty">
		<rdfs:subClassOf rdf:resource="https://spec.edmcouncil.org/fibo/FBC/DebtAndEquities/Guaranty/Guaranty"/>
		<rdfs:subClassOf>
			<owl:Restriction>
				<owl:onProperty rdf:resource="&fibo-sec-dbt-dbt-gty;takesFormOfCollateral"/>
				<owl:someValuesFrom rdf:resource="https://spec.edmcouncil.org/fibo/FBC/DebtAndEquities/Debt/Collateral"/>
			</owl:Restriction>
		</rdfs:subClassOf>
		<rdfs:label xml:lang="en">collateralized guaranty</rdfs:label>
		<skos:definition xml:lang="en">Guaranty which takes the form of some Collateral. e.g. if a Security is guaranteed by collateral, assets (the Collateral) are pledged to a lender until a loan is repaid.</skos:definition>
		<skos:editorialNote xml:lang="en">Some models have Collateral as a type of Guaranty, but actually it is a way of mechanizing the Guaranty and is not the same type of Thing. Details: Seems that in collateralized guaranty you are asking for some collateral from the Guarantor. So this distinguishes it from what is just a Collateral. The process is that the guarantor offers something, the lender might say this is not adequate and will ask for additional collateral. CollateralDefinition Origin:FIBIM Extended</skos:editorialNote>
	</owl:Class>
	
	<owl:Class rdf:about="&fibo-sec-dbt-dbt-gty;GovernmentGuaranty">
		<rdfs:subClassOf rdf:resource="https://spec.edmcouncil.org/fibo/FBC/DebtAndEquities/Guaranty/Guaranty"/>
		<rdfs:subClassOf>
			<owl:Restriction>
				<owl:onProperty rdf:resource="https://spec.edmcouncil.org/fibo/FBC/DebtAndEquities/Guaranty/isGuaranteedBy"/>
				<owl:someValuesFrom rdf:resource="&fibo-sec-dbt-dbt-gty;StateGuarantor"/>
			</owl:Restriction>
		</rdfs:subClassOf>
		<rdfs:label xml:lang="en">government guaranty</rdfs:label>
		<skos:definition xml:lang="en">Guaranty is provided by a government, e.g. a security is guaranteed by a Government.</skos:definition>
	</owl:Class>
	
	<owl:Class rdf:about="&fibo-sec-dbt-dbt-gty;InsuranceBackedGuaranty">
		<rdfs:subClassOf rdf:resource="https://spec.edmcouncil.org/fibo/FBC/DebtAndEquities/Guaranty/Guaranty"/>
		<rdfs:subClassOf>
			<owl:Restriction>
				<owl:onProperty rdf:resource="&fibo-sec-dbt-dbt-gtyx;guarantyTakesFormOf"/>
				<owl:someValuesFrom rdf:resource="&fibo-sec-dbt-dbt-gty;SecuritiesGuarantyInsurancePolicy"/>
			</owl:Restriction>
		</rdfs:subClassOf>
		<rdfs:label xml:lang="en">insurance backed guaranty</rdfs:label>
		<skos:definition xml:lang="en">Security is guaranteed by an insurance policy.</skos:definition>
	</owl:Class>
	
	<owl:Class rdf:about="&fibo-sec-dbt-dbt-gty;JointGuaranty">
		<rdfs:subClassOf rdf:resource="https://spec.edmcouncil.org/fibo/FBC/DebtAndEquities/Guaranty/Guaranty"/>
		<rdfs:subClassOf>
			<owl:Restriction>
				<owl:onProperty rdf:resource="https://spec.edmcouncil.org/fibo/FBC/DebtAndEquities/Guaranty/isGuaranteedBy"/>
				<owl:onClass rdf:resource="&fibo-sec-dbt-dbt-gtyx;ContractGuarantor"/>
				<owl:qualifiedCardinality rdf:datatype="&xsd;nonNegativeInteger">2</owl:qualifiedCardinality>
			</owl:Restriction>
		</rdfs:subClassOf>
		<rdfs:label xml:lang="en">joint guaranty</rdfs:label>
		<skos:definition xml:lang="en">Guaranty provided by two or more parties jointly and severally.</skos:definition>
	</owl:Class>
	
	<owl:Class rdf:about="&fibo-sec-dbt-dbt-gty;LetterOfCredit">
		<rdfs:subClassOf rdf:resource="&fibo-fnd-inf-inf;WrittenInformation"/>
		<rdfs:subClassOf>
			<owl:Restriction>
				<owl:onProperty rdf:resource="&fibo-sec-dbt-dbt-gty;issuedBy"/>
				<owl:someValuesFrom rdf:resource="&fibo-sec-dbt-dbt-gty;LetterOfCreditIssuer"/>
			</owl:Restriction>
		</rdfs:subClassOf>
		<rdfs:label xml:lang="en">letter of credit</rdfs:label>
		<skos:definition xml:lang="en">A letter from a bank or other creditworthy institution setting out the holder&apos;s ability to access credit.</skos:definition>
		<skos:editorialNote xml:lang="en">It should be possible to source a formal, legal definition for this.</skos:editorialNote>
	</owl:Class>
	
	<owl:Class rdf:about="&fibo-sec-dbt-dbt-gty;LetterOfCreditGuaranty">
		<rdfs:subClassOf rdf:resource="https://spec.edmcouncil.org/fibo/FBC/DebtAndEquities/Guaranty/Guaranty"/>
		<rdfs:subClassOf>
			<owl:Restriction>
				<owl:onProperty rdf:resource="&fibo-sec-dbt-dbt-gtyx;guarantyTakesFormOf"/>
				<owl:someValuesFrom rdf:resource="&fibo-sec-dbt-dbt-gty;LetterOfCredit"/>
			</owl:Restriction>
		</rdfs:subClassOf>
		<rdfs:label xml:lang="en">letter of credit guaranty</rdfs:label>
		<skos:definition xml:lang="en">Guaranty takes the form of a letter of credit, ie, a document issued by a bank guaranteeing the payment up to a stated amount for a specified period.</skos:definition>
	</owl:Class>
	
	<owl:Class rdf:about="&fibo-sec-dbt-dbt-gty;LetterOfCreditIssuer">
		<rdfs:subClassOf rdf:resource="&fibo-fnd-pty-pty;PartyInRole"/>
		<rdfs:label xml:lang="en">letter of credit issuer</rdfs:label>
		<skos:definition xml:lang="en">The party which issues a Letter of Credit.</skos:definition>
		<skos:editorialNote xml:lang="en">Term added by inspection of the ISO 20022 FIBIM terms and definitions.</skos:editorialNote>
	</owl:Class>
	
	<owl:Class rdf:about="&fibo-sec-dbt-dbt-gty;LienGuaranty">
		<rdfs:subClassOf rdf:resource="https://spec.edmcouncil.org/fibo/FBC/DebtAndEquities/Guaranty/Guaranty"/>
		<rdfs:subClassOf>
			<owl:Restriction>
				<owl:onProperty rdf:resource="&fibo-sec-dbt-dbt-gty;lien"/>
				<owl:someValuesFrom rdf:resource="&fibo-fnd-plcx-re;RealEstate"/>
			</owl:Restriction>
		</rdfs:subClassOf>
		<rdfs:label xml:lang="en">lien guaranty</rdfs:label>
		<skos:definition xml:lang="en">Guaranty takes the form of a lien, that is a creditor&apos;s claim against property, eg, a mortgage is a lien against a house.</skos:definition>
		<skos:editorialNote xml:lang="en">Looks like this should be a child of &quot;Collateralized Guaranty&quot; but we need to research this further. Or they may in fact be the same meaning, or we may need to look at the collateral contract. Look at the collateral contract for the asset, which says &quot;I am going to deliver this asset as settlement for the loan&quot;. the &quot;I&quot; is the Guarantor if it&apos;s a kind of collateralized guaranty, and it&apos;s the Borrower if it&apos;s just Collateral on the Loan. Effectively the Guarantor becomes like theb borrower in terms of being who is chased for the loan amount outsstanding. For instances, differences between how you would foreclose on a moartgage between the US and Commonwealth countries. Relates to how you take ownership of the asset.</skos:editorialNote>
	</owl:Class>
	
	<owl:Class rdf:about="&fibo-sec-dbt-dbt-gty;NegativePledge">
		<rdfs:subClassOf rdf:resource="https://spec.edmcouncil.org/fibo/FBC/DebtAndEquities/Guaranty/Guaranty"/>
		<rdfs:label xml:lang="en">negative pledge</rdfs:label>
		<skos:definition xml:lang="en">Guaranty whereby the issuer will not pledge any assets if doing so would result in less security for the investors.</skos:definition>
		<skos:editorialNote xml:lang="en">This also exists in loans, so revise the wording to reflect this. Also clarify that the pledge to one potential lender is not to pledge assets to some other potential lender at some time in the future. These are often broken. An agreement which gives someone a right to seize those assets? No, that&apos;s implicit in the loan i.e. secured loan. So the pledge does not introduce anything with any new legal standing, other than that having broken the pledge, you have de facto defauled on the loan even if you have not default ed on laon payments. It gies the lender the right to recall the loan as there is a technical default when this happens.</skos:editorialNote>
	</owl:Class>
	
	<owl:Class rdf:about="&fibo-sec-dbt-dbt-gty;SecuritiesGuarantyInsurancePolicy">
		<rdfs:subClassOf rdf:resource="&fibo-fnd-inf-doc;InsurancePolicy"/>
		<rdfs:label xml:lang="en">securities guaranty insurance policy</rdfs:label>
		<skos:definition xml:lang="en">Some policy by which some party (directly or more usually through an intermediary who writes this policy) agrees to cover some risk as identified in this policy, on behalf of the holder of the policy. further Notes: Added specifically to cover financial instruments modeling of insurance backed Guaranty. This term would belong within a separate section of specialist insurance terms if there were such a section.</skos:definition>
	</owl:Class>
	
	<owl:Class rdf:about="&fibo-sec-dbt-dbt-gty;SimpleGuaranty">
		<rdfs:subClassOf rdf:resource="https://spec.edmcouncil.org/fibo/FBC/DebtAndEquities/Guaranty/Guaranty"/>
		<rdfs:label xml:lang="en">simple guaranty</rdfs:label>
		<skos:definition xml:lang="en">No definition</skos:definition>
	</owl:Class>
	
	<owl:Class rdf:about="&fibo-sec-dbt-dbt-gty;StateGuarantor">
		<rdfs:subClassOf rdf:resource="https://spec.edmcouncil.org/fibo/FBC/DebtAndEquities/Guaranty/Guarantor"/>
		<rdfs:subClassOf>
			<owl:Restriction>
				<owl:onProperty rdf:resource="&fibo-sec-dbt-dbt-gty;identifiedAs"/>
				<owl:someValuesFrom rdf:resource="&fibo-be-ge-ge;SovereignState"/>
			</owl:Restriction>
		</rdfs:subClassOf>
		<rdfs:label xml:lang="en">state guarantor</rdfs:label>
		<skos:definition xml:lang="en">A State, acting as Party to some participatory context such as issuance, guaranty provision.</skos:definition>
	</owl:Class>
	
	<owl:ObjectProperty rdf:about="&fibo-sec-dbt-dbt-gty;identifiedAs">
		<rdfs:subPropertyOf rdf:resource="&fibo-sec-dbt-dbt-gtyx;guarantorHasIdentity"/>
		<rdfs:label xml:lang="en">identified as</rdfs:label>
		<rdfs:domain rdf:resource="&fibo-sec-dbt-dbt-gty;StateGuarantor"/>
		<rdfs:range rdf:resource="&fibo-be-ge-ge;SovereignState"/>
	</owl:ObjectProperty>
	
	<owl:ObjectProperty rdf:about="&fibo-sec-dbt-dbt-gty;issuedBy">
		<rdfs:label xml:lang="en">issued by</rdfs:label>
		<rdfs:domain rdf:resource="&fibo-sec-dbt-dbt-gty;LetterOfCredit"/>
		<rdfs:range rdf:resource="&fibo-sec-dbt-dbt-gty;LetterOfCreditIssuer"/>
	</owl:ObjectProperty>
	
	<owl:ObjectProperty rdf:about="&fibo-sec-dbt-dbt-gty;lien">
		<rdfs:subPropertyOf rdf:resource="&fibo-sec-dbt-dbt-gtyx;guarantyTakesFormOf"/>
		<rdfs:label xml:lang="en">is encumbrance on</rdfs:label>
		<rdfs:domain rdf:resource="&fibo-sec-dbt-dbt-gty;LienGuaranty"/>
		<rdfs:range rdf:resource="&fibo-fnd-plcx-re;RealEstate"/>
	</owl:ObjectProperty>
	
	<owl:ObjectProperty rdf:about="&fibo-sec-dbt-dbt-gty;loCDetails">
		<rdfs:label xml:lang="en">lo c details</rdfs:label>
		<rdfs:domain rdf:resource="&fibo-sec-dbt-dbt-gty;LetterOfCreditGuaranty"/>
		<rdfs:range rdf:resource="&fibo-fnd-utl-val;TextValue"/>
		<skos:definition xml:lang="en">Details of the Letter of Credit</skos:definition>
	</owl:ObjectProperty>
	
	<owl:ObjectProperty rdf:about="&fibo-sec-dbt-dbt-gty;policyDetails">
		<rdfs:label xml:lang="en">policy details</rdfs:label>
		<rdfs:domain rdf:resource="&fibo-sec-dbt-dbt-gty;InsuranceBackedGuaranty"/>
		<rdfs:range rdf:resource="&fibo-fnd-utl-val;TextValue"/>
		<skos:definition xml:lang="en">Details of the Insurance Policy which make up this Guaranty.</skos:definition>
	</owl:ObjectProperty>
	
	<owl:ObjectProperty rdf:about="&fibo-sec-dbt-dbt-gty;takesFormOfCollateral">
		<rdfs:subPropertyOf rdf:resource="&fibo-sec-dbt-dbt-gtyx;guarantyTakesFormOf"/>
		<rdfs:label xml:lang="en">takes form of collateral</rdfs:label>
		<rdfs:domain rdf:resource="&fibo-sec-dbt-dbt-gty;CollateralizedGuaranty"/>
		<rdfs:range rdf:resource="https://spec.edmcouncil.org/fibo/FBC/DebtAndEquities/Debt/Collateral"/>
	</owl:ObjectProperty>

</rdf:RDF>