<?xml version="1.0" encoding="UTF-8"?>
<!DOCTYPE rdf:RDF [
	<!ENTITY dct "http://purl.org/dc/terms/">
	<!ENTITY fibo-be-fct-fct "https://spec.edmcouncil.org/fibo/BE/FunctionalEntities/FunctionalEntities/">
	<!ENTITY fibo-be-ge-ge "https://spec.edmcouncil.org/fibo/BE/GovernmentEntities/GovernmentEntities/">
	<!ENTITY fibo-be-plc-plc "https://spec.edmcouncil.org/fibo/BE/PrivateLimitedCompanies/PrivateLimitedCompanies/">
	<!ENTITY fibo-be-ptr-ptr "https://spec.edmcouncil.org/fibo/BE/Partnerships/Partnerships/">
	<!ENTITY fibo-fbc-fct-ra "https://spec.edmcouncil.org/fibo/FBC/FunctionalEntities/RegistrationAuthorities/">
	<!ENTITY fibo-fbc-fct-rga "https://spec.edmcouncil.org/fibo/FBC/FunctionalEntities/RegulatoryAgencies/">
	<!ENTITY fibo-fbc-fi-fi "https://spec.edmcouncil.org/fibo/FBC/FinancialInstruments/FinancialInstruments/">
	<!ENTITY fibo-fbc-pas-fpas "https://spec.edmcouncil.org/fibo/FBC/ProductsAndServices/FinancialProductsAndServices/">
	<!ENTITY fibo-fnd-aap-agt "https://spec.edmcouncil.org/fibo/FND/AgentsAndPeople/Agents/">
	<!ENTITY fibo-fnd-arr-id "https://spec.edmcouncil.org/fibo/FND/Arrangements/IdentifiersAndIndices/">
	<!ENTITY fibo-fnd-law-jur "https://spec.edmcouncil.org/fibo/FND/Law/Jurisdiction/">
	<!ENTITY fibo-fnd-rel-rel "https://spec.edmcouncil.org/fibo/FND/Relations/Relations/">
	<!ENTITY fibo-fnd-utl-av "https://spec.edmcouncil.org/fibo/FND/Utilities/AnnotationVocabulary/">
	<!ENTITY fibo-ind-ind-ind "https://spec.edmcouncil.org/fibo/IND/Indicators/Indicators/">
	<!ENTITY fibo-sec-sec-id "https://spec.edmcouncil.org/fibo/SEC/Securities/SecuritiesIdentification/">
	<!ENTITY fibo-sec-sec-lst "https://spec.edmcouncil.org/fibo/SEC/Securities/SecuritiesListings/">
	<!ENTITY owl "http://www.w3.org/2002/07/owl#">
	<!ENTITY rdf "http://www.w3.org/1999/02/22-rdf-syntax-ns#">
	<!ENTITY rdfs "http://www.w3.org/2000/01/rdf-schema#">
	<!ENTITY skos "http://www.w3.org/2004/02/skos/core#">
	<!ENTITY sm "http://www.omg.org/techprocess/ab/SpecificationMetadata/">
	<!ENTITY xsd "http://www.w3.org/2001/XMLSchema#">
]>
<rdf:RDF
	xml:base="https://spec.edmcouncil.org/fibo/SEC/Securities/SecuritiesIdentification/"
	xmlns:dct="http://purl.org/dc/terms/"
	xmlns:fibo-be-fct-fct="https://spec.edmcouncil.org/fibo/BE/FunctionalEntities/FunctionalEntities/"
	xmlns:fibo-be-ge-ge="https://spec.edmcouncil.org/fibo/BE/GovernmentEntities/GovernmentEntities/"
	xmlns:fibo-be-plc-plc="https://spec.edmcouncil.org/fibo/BE/PrivateLimitedCompanies/PrivateLimitedCompanies/"
	xmlns:fibo-be-ptr-ptr="https://spec.edmcouncil.org/fibo/BE/Partnerships/Partnerships/"
	xmlns:fibo-fbc-fct-ra="https://spec.edmcouncil.org/fibo/FBC/FunctionalEntities/RegistrationAuthorities/"
	xmlns:fibo-fbc-fct-rga="https://spec.edmcouncil.org/fibo/FBC/FunctionalEntities/RegulatoryAgencies/"
	xmlns:fibo-fbc-fi-fi="https://spec.edmcouncil.org/fibo/FBC/FinancialInstruments/FinancialInstruments/"
	xmlns:fibo-fbc-pas-fpas="https://spec.edmcouncil.org/fibo/FBC/ProductsAndServices/FinancialProductsAndServices/"
	xmlns:fibo-fnd-aap-agt="https://spec.edmcouncil.org/fibo/FND/AgentsAndPeople/Agents/"
	xmlns:fibo-fnd-arr-id="https://spec.edmcouncil.org/fibo/FND/Arrangements/IdentifiersAndIndices/"
	xmlns:fibo-fnd-law-jur="https://spec.edmcouncil.org/fibo/FND/Law/Jurisdiction/"
	xmlns:fibo-fnd-rel-rel="https://spec.edmcouncil.org/fibo/FND/Relations/Relations/"
	xmlns:fibo-fnd-utl-av="https://spec.edmcouncil.org/fibo/FND/Utilities/AnnotationVocabulary/"
	xmlns:fibo-ind-ind-ind="https://spec.edmcouncil.org/fibo/IND/Indicators/Indicators/"
	xmlns:fibo-sec-sec-id="https://spec.edmcouncil.org/fibo/SEC/Securities/SecuritiesIdentification/"
	xmlns:fibo-sec-sec-lst="https://spec.edmcouncil.org/fibo/SEC/Securities/SecuritiesListings/"
	xmlns:owl="http://www.w3.org/2002/07/owl#"
	xmlns:rdf="http://www.w3.org/1999/02/22-rdf-syntax-ns#"
	xmlns:rdfs="http://www.w3.org/2000/01/rdf-schema#"
	xmlns:skos="http://www.w3.org/2004/02/skos/core#"
	xmlns:sm="http://www.omg.org/techprocess/ab/SpecificationMetadata/"
	xmlns:xsd="http://www.w3.org/2001/XMLSchema#">
	
	<owl:Ontology
		rdf:about="https://spec.edmcouncil.org/fibo/SEC/Securities/SecuritiesIdentification/">
		<rdfs:label>Securities Identification Ontology</rdfs:label>
		<dct:license
			rdf:resource="&sm;MITLicense"/>
		<sm:contentLanguage
			rdf:resource="http://www.omg.org/spec/ODM/"/>
		<sm:contentLanguage
			rdf:resource="http://www.w3.org/standards/techs/owl#w3c_all"/>
		<sm:copyright>Copyright (c) 2016-2017 EDM Council, Inc.
Copyright (c) 2016-2017 Object Management Group, Inc.</sm:copyright>
		<sm:dependsOn
			rdf:resource="https://spec.edmcouncil.org/fibo/BE/"/>
		<sm:dependsOn
			rdf:resource="https://spec.edmcouncil.org/fibo/FBC/"/>
		<sm:dependsOn
			rdf:resource="https://spec.edmcouncil.org/fibo/FND/"/>
		<sm:dependsOn
			rdf:resource="https://spec.edmcouncil.org/fibo/IND/"/>
		<sm:dependsOn
			rdf:resource="https://spec.edmcouncil.org/fibo/SEC/Securities/SecuritiesClassification/"/>
		<sm:dependsOn
			rdf:resource="https://spec.edmcouncil.org/fibo/SEC/Securities/SecuritiesListings/"/>
		<sm:fileAbbreviation>fibo-sec-sec-id</sm:fileAbbreviation>
		<sm:fileAbstract>This ontology defines concepts required to identify securities, including a number of well-known securities identifiers and related schemes, registries, and registration authorities.</sm:fileAbstract>
		<sm:filename>SecuritiesIdentification.rdf</sm:filename>
		<rdfs:seeAlso
			rdf:resource="https://spec.edmcouncil.org/fibo/AboutTheEDMC-FIBOFamily/"/>
		<rdfs:seeAlso
			rdf:resource="https://spec.edmcouncil.org/fibo/SEC/AboutSEC/"/>
		<rdfs:seeAlso
			rdf:resource="https://spec.edmcouncil.org/fibo/SEC/Securities/AboutSecurities/"/>
		<owl:imports
			rdf:resource="https://spec.edmcouncil.org/fibo/BE/FunctionalEntities/FunctionalEntities/"/>
		<owl:imports
			rdf:resource="https://spec.edmcouncil.org/fibo/BE/GovernmentEntities/GovernmentEntities/"/>
		<owl:imports
			rdf:resource="https://spec.edmcouncil.org/fibo/BE/Partnerships/Partnerships/"/>
		<owl:imports
			rdf:resource="https://spec.edmcouncil.org/fibo/BE/PrivateLimitedCompanies/PrivateLimitedCompanies/"/>
		<owl:imports
			rdf:resource="https://spec.edmcouncil.org/fibo/FBC/FinancialInstruments/FinancialInstruments/"/>
		<owl:imports
			rdf:resource="https://spec.edmcouncil.org/fibo/FBC/FunctionalEntities/RegistrationAuthorities/"/>
		<owl:imports
			rdf:resource="https://spec.edmcouncil.org/fibo/FBC/FunctionalEntities/RegulatoryAgencies/"/>
		<owl:imports
			rdf:resource="https://spec.edmcouncil.org/fibo/FBC/ProductsAndServices/FinancialProductsAndServices/"/>
		<owl:imports
			rdf:resource="https://spec.edmcouncil.org/fibo/FND/AgentsAndPeople/Agents/"/>
		<owl:imports
			rdf:resource="https://spec.edmcouncil.org/fibo/FND/Arrangements/IdentifiersAndIndices/"/>
		<owl:imports
			rdf:resource="https://spec.edmcouncil.org/fibo/FND/Law/Jurisdiction/"/>
		<owl:imports
			rdf:resource="https://spec.edmcouncil.org/fibo/FND/Relations/Relations/"/>
		<owl:imports
			rdf:resource="https://spec.edmcouncil.org/fibo/FND/Utilities/AnnotationVocabulary/"/>
		<owl:imports
			rdf:resource="https://spec.edmcouncil.org/fibo/IND/Indicators/Indicators/"/>
		<owl:imports
			rdf:resource="https://spec.edmcouncil.org/fibo/SEC/Securities/SecuritiesListings/"/>
		<owl:versionIRI
			rdf:resource="https://spec.edmcouncil.org/fibo/SEC/20170201/Securities/SecuritiesIdentification/"/>
	</owl:Ontology>
	
	<fibo-be-ptr-ptr:Partnership
		rdf:about="&fibo-sec-sec-id;BloombergLP">
		<rdf:type
			rdf:resource="&owl;NamedIndividual"/>
		<rdfs:label>Bloomberg LP</rdfs:label>
		<rdfs:seeAlso
			rdf:resource="http://www.bloomberg.com/"/>
		<skos:definition>individual representing the Bloomberg LP legal entity, which is a global business and financial information services and news provider as well as a FIGI registration authority</skos:definition>
		<fibo-fnd-rel-rel:hasLegalName>Bloomberg L.P.</fibo-fnd-rel-rel:hasLegalName>
	</fibo-be-ptr-ptr:Partnership>
	
	<fibo-sec-sec-id:NationalSecuritiesIdentifyingNumberRegistry
		rdf:about="&fibo-sec-sec-id;CGSCUSIPAccessRepository">
		<rdf:type
			rdf:resource="&owl;NamedIndividual"/>
		<rdfs:label>CGS CUSIP Access Repository</rdfs:label>
		<rdfs:seeAlso
			rdf:resource="https://www.cusip.com/cusip/index.htm"/>
		<skos:definition>individual representing the CGS (CUSIP Global Services) CUSIP Access services and repository, a proprietary repository of security identifiers, issued by CUSIP Global Services, that is the National Securities Identifying Number (NSIN) for securities issued in North America, which is also part of the ISIN for the security it identifies</skos:definition>
		<fibo-fnd-rel-rel:isManagedBy
			rdf:resource="&fibo-sec-sec-id;CUSIPGlobalServices"/>
	</fibo-sec-sec-id:NationalSecuritiesIdentifyingNumberRegistry>
	
	<rdf:Description
		rdf:about="&fibo-sec-sec-id;CUSIPGlobalServices">
		<rdf:type
			rdf:resource="&owl;NamedIndividual"/>
		<rdf:type
			rdf:resource="&fibo-fbc-pas-fpas;FinancialServiceProvider"/>
		<rdf:type
			rdf:resource="&fibo-ind-ind-ind;FinancialInformationPublisher"/>
		<rdf:type
			rdf:resource="&fibo-sec-sec-id;NationalNumberingAgency"/>
		<rdfs:label>CUSIP Global Services</rdfs:label>
		<rdfs:seeAlso
			rdf:resource="http://www.cusip.com/"/>
		<skos:definition>individual representing the CUSIP Global Services financial services provider that is the national numbering agency (NNA) for CUSIPs in North America</skos:definition>
		<fibo-fbc-fct-ra:registers
			rdf:resource="&fibo-sec-sec-id;CommitteeOnUniformSecuritiesIdentificationProceduresNumber"/>
		<fibo-fnd-rel-rel:hasIdentity
			rdf:resource="&fibo-sec-sec-id;SPGlobalMarketIntelligence"/>
	</rdf:Description>
	
	<owl:Class
		rdf:about="&fibo-sec-sec-id;CUSIPInternationalNumberingSystemNumber">
		<rdfs:subClassOf
			rdf:resource="&fibo-sec-sec-id;ProprietarySecurityIdentifier"/>
		<rdfs:subClassOf>
			<owl:Restriction>
				<owl:hasValue
					rdf:resource="&fibo-sec-sec-id;CGSCUSIPAccessRepository"/>
				<owl:onProperty
					rdf:resource="&fibo-fbc-fct-ra;isRegisteredIn"/>
			</owl:Restriction>
		</rdfs:subClassOf>
		<rdfs:subClassOf>
			<owl:Restriction>
				<owl:hasValue
					rdf:resource="&fibo-sec-sec-id;CUSIPGlobalServices"/>
				<owl:onProperty
					rdf:resource="&fibo-fbc-fct-ra;isRegisteredBy"/>
			</owl:Restriction>
		</rdfs:subClassOf>
		<rdfs:subClassOf>
			<owl:Restriction>
				<owl:hasValue
					rdf:resource="&fibo-sec-sec-id;CUSIPInternationalNumberingSystemScheme"/>
				<owl:onProperty
					rdf:resource="&fibo-fnd-rel-rel;hasDefinition"/>
			</owl:Restriction>
		</rdfs:subClassOf>
		<rdfs:label>CUSIP International Numbering System (CINS) number</rdfs:label>
		<rdfs:seeAlso
			rdf:resource="http://isin.net/cins/"/>
		<skos:definition>a 9-character alphanumeric identifier that employs the same 9 characters as CUSIP, but also contains a letter of the alphabet in the first position signifying the issuer&apos;s country or geographic region, issued by CUSIP Global Services</skos:definition>
		<fibo-fnd-utl-av:abbreviation>CINS number</fibo-fnd-utl-av:abbreviation>
		<fibo-fnd-utl-av:adaptedFrom
			rdf:datatype="&xsd;anyURI">http://www.investopedia.com/terms/c/cins.asp</fibo-fnd-utl-av:adaptedFrom>
		<fibo-fnd-utl-av:adaptedFrom
			rdf:datatype="&xsd;anyURI">https://www.cusip.com/cusip/about-cgs-identifiers.htm</fibo-fnd-utl-av:adaptedFrom>
	</owl:Class>
	
	<fibo-sec-sec-id:ProprietarySecurityIdentificationScheme
		rdf:about="&fibo-sec-sec-id;CUSIPInternationalNumberingSystemScheme">
		<rdf:type
			rdf:resource="&owl;NamedIndividual"/>
		<rdfs:label>CUSIP International Numbering System (CINS) scheme</rdfs:label>
		<skos:definition>a security identification scheme that extends the CUSIP scheme, used to identify securities outside of the United States and Canada for the purposes of facilitating clearing and settlement of trades</skos:definition>
		<fibo-fnd-rel-rel:defines
			rdf:resource="&fibo-sec-sec-id;CUSIPInternationalNumberingSystemSchemeNumber"/>
		<fibo-fnd-utl-av:abbreviation>CINS scheme</fibo-fnd-utl-av:abbreviation>
		<fibo-fnd-utl-av:adaptedFrom
			rdf:datatype="&xsd;anyURI">https://www.cusip.com/cusip/about-cgs-identifiers.htm</fibo-fnd-utl-av:adaptedFrom>
	</fibo-sec-sec-id:ProprietarySecurityIdentificationScheme>
	
	<owl:Class
		rdf:about="&fibo-sec-sec-id;CUSIPInternationalNumberingSystemSchemeNumber">
		<rdfs:label>cusipinternational numbering system scheme number</rdfs:label>
	</owl:Class>
	
	<owl:Class
		rdf:about="&fibo-sec-sec-id;CommitteeOnUniformSecuritiesIdentificationProceduresNumber">
		<rdfs:subClassOf
			rdf:resource="&fibo-sec-sec-id;NationalSecuritiesIdentifyingNumber"/>
		<rdfs:subClassOf
			rdf:resource="&fibo-sec-sec-id;ProprietarySecurityIdentifier"/>
		<rdfs:subClassOf>
			<owl:Restriction>
				<owl:hasValue
					rdf:resource="&fibo-sec-sec-id;CGSCUSIPAccessRepository"/>
				<owl:onProperty
					rdf:resource="&fibo-fbc-fct-ra;isRegisteredIn"/>
			</owl:Restriction>
		</rdfs:subClassOf>
		<rdfs:subClassOf>
			<owl:Restriction>
				<owl:hasValue
					rdf:resource="&fibo-sec-sec-id;CUSIPGlobalServices"/>
				<owl:onProperty
					rdf:resource="&fibo-fbc-fct-ra;isRegisteredBy"/>
			</owl:Restriction>
		</rdfs:subClassOf>
		<rdfs:subClassOf>
			<owl:Restriction>
				<owl:hasValue
					rdf:resource="&fibo-sec-sec-id;CommitteeOnUniformSecuritiesIdentificationProceduresScheme"/>
				<owl:onProperty
					rdf:resource="&fibo-fnd-rel-rel;hasDefinition"/>
			</owl:Restriction>
		</rdfs:subClassOf>
		<rdfs:label>Committee on Uniform Securities Identification Procedures (CUSIP) number</rdfs:label>
		<rdfs:seeAlso
			rdf:resource="https://www.cusip.com/cusip/about-cgs-identifiers.htm"/>
		<skos:definition>a nine-character alphanumeric number that identifies all North American stocks and registered bonds for the purposes of facilitating clearing and settlement of trades, issued by CUSIP Global Services on behalf of the American Bankers&apos; Association, which is a part of Standard and Poor&apos;s Capital IQ, that is the National Numbering Agency Identifier for securities issued in North America, which is also part of the ISIN for the security it identifies</skos:definition>
		<fibo-fnd-utl-av:abbreviation>CUSIP number</fibo-fnd-utl-av:abbreviation>
		<fibo-fnd-utl-av:adaptedFrom>Barron&apos;s Dictionary of Finance and Investment Terms, Ninth Edition, 2014</fibo-fnd-utl-av:adaptedFrom>
	</owl:Class>
	
	<rdf:Description
		rdf:about="&fibo-sec-sec-id;CommitteeOnUniformSecuritiesIdentificationProceduresScheme">
		<rdf:type
			rdf:resource="&owl;NamedIndividual"/>
		<rdf:type
			rdf:resource="&fibo-sec-sec-id;NationalSecurityIdentificationScheme"/>
		<rdf:type
			rdf:resource="&fibo-sec-sec-id;ProprietarySecurityIdentificationScheme"/>
		<rdfs:label>Committee on Uniform Securities Identification Procedures (CUSIP) scheme</rdfs:label>
		<rdfs:seeAlso
			rdf:resource="https://www.cusip.com/cusip/about-cgs-identifiers.htm"/>
		<skos:definition>a national security identification scheme used to identify all North American stocks and registered bonds for the purposes of facilitating clearing and settlement of trades</skos:definition>
		<fibo-fnd-rel-rel:defines
			rdf:resource="&fibo-sec-sec-id;CommitteeOnUniformSecuritiesIdentificationProceduresNumber"/>
		<fibo-fnd-utl-av:abbreviation>CUSIP scheme</fibo-fnd-utl-av:abbreviation>
		<fibo-fnd-utl-av:adaptedFrom>Barron&apos;s Dictionary of Finance and Investment Terms, Ninth Edition, 2014</fibo-fnd-utl-av:adaptedFrom>
	</rdf:Description>
	
	<fibo-sec-sec-id:SecurityIdentificationScheme
		rdf:about="&fibo-sec-sec-id;EuroclearIDScheme">
		<rdf:type
			rdf:resource="&owl;NamedIndividual"/>
	</fibo-sec-sec-id:SecurityIdentificationScheme>
	
	<owl:Class
		rdf:about="&fibo-sec-sec-id;ExchangeSpecificSecuritiesRegistry">
		<rdfs:subClassOf
			rdf:resource="&fibo-fbc-fct-ra;Registry"/>
		<rdfs:subClassOf>
			<owl:Restriction>
				<owl:allValuesFrom
					rdf:resource="&fibo-sec-sec-id;ExchangeSpecificSecuritiesRegistryEntry"/>
				<owl:onProperty
					rdf:resource="&fibo-fbc-fct-ra;hasRegistryEntry"/>
			</owl:Restriction>
		</rdfs:subClassOf>
		<rdfs:subClassOf>
			<owl:Restriction>
				<owl:onClass
					rdf:resource="&fibo-sec-sec-id;ExchangeSpecificSecurityIdentificationScheme"/>
				<owl:onProperty
					rdf:resource="&fibo-be-fct-fct;isCharacterizedBy"/>
				<owl:qualifiedCardinality
					rdf:datatype="&xsd;nonNegativeInteger">1</owl:qualifiedCardinality>
			</owl:Restriction>
		</rdfs:subClassOf>
		<rdfs:subClassOf>
			<owl:Restriction>
				<owl:onProperty
					rdf:resource="&fibo-fnd-rel-rel;isManagedBy"/>
				<owl:someValuesFrom
					rdf:resource="&fibo-sec-sec-lst;SecuritiesExchange"/>
			</owl:Restriction>
		</rdfs:subClassOf>
		<rdfs:label>exchange-specific securities registry</rdfs:label>
		<skos:definition>a registry used by a securities exchange in managing the security identifiers and related information that it registers and manages</skos:definition>
	</owl:Class>
	
	<owl:Class
		rdf:about="&fibo-sec-sec-id;ExchangeSpecificSecuritiesRegistryEntry">
		<rdfs:subClassOf
			rdf:resource="&fibo-fbc-fct-ra;RegistryEntry"/>
		<rdfs:subClassOf>
			<owl:Restriction>
				<owl:allValuesFrom
					rdf:resource="&fibo-sec-sec-id;ExchangeSpecificSecuritiesRegistry"/>
				<owl:onProperty
					rdf:resource="&fibo-fbc-pas-fpas;isConstituentOf"/>
			</owl:Restriction>
		</rdfs:subClassOf>
		<rdfs:subClassOf>
			<owl:Restriction>
				<owl:allValuesFrom
					rdf:resource="&fibo-sec-sec-lst;ListedSecurity"/>
				<owl:onProperty
					rdf:resource="&fibo-fnd-rel-rel;appliesTo"/>
			</owl:Restriction>
		</rdfs:subClassOf>
		<rdfs:subClassOf>
			<owl:Restriction>
				<owl:onProperty
					rdf:resource="&fibo-fnd-rel-rel;comprises"/>
				<owl:someValuesFrom
					rdf:resource="&fibo-sec-sec-id;ListedSecurityIdentifier"/>
			</owl:Restriction>
		</rdfs:subClassOf>
		<rdfs:label>exchange-specific securities registry entry</rdfs:label>
		<skos:definition>an entry in an exchange-specific securities repository</skos:definition>
	</owl:Class>
	
	<owl:Class
		rdf:about="&fibo-sec-sec-id;ExchangeSpecificSecurityIdentificationScheme">
		<rdfs:subClassOf
			rdf:resource="&fibo-fbc-fct-ra;RegistrationScheme"/>
		<rdfs:subClassOf
			rdf:resource="&fibo-sec-sec-id;SecurityIdentificationScheme"/>
		<rdfs:subClassOf>
			<owl:Restriction>
				<owl:allValuesFrom
					rdf:resource="&fibo-sec-sec-id;ListedSecurityIdentifier"/>
				<owl:onProperty
					rdf:resource="&fibo-fnd-rel-rel;defines"/>
			</owl:Restriction>
		</rdfs:subClassOf>
		<rdfs:subClassOf>
			<owl:Restriction>
				<owl:onProperty
					rdf:resource="&fibo-fnd-rel-rel;characterizes"/>
				<owl:someValuesFrom
					rdf:resource="&fibo-sec-sec-id;ExchangeSpecificSecuritiesRegistry"/>
			</owl:Restriction>
		</rdfs:subClassOf>
		<rdfs:label>exchange-specific security identification scheme</rdfs:label>
		<skos:definition>an identification scheme used by a securities exchange in issuing security identifiers</skos:definition>
	</owl:Class>
	
	<fibo-sec-sec-id:ProprietarySecurityIdentificationScheme
		rdf:about="&fibo-sec-sec-id;FTIDScheme">
		<rdf:type
			rdf:resource="&owl;NamedIndividual"/>
	</fibo-sec-sec-id:ProprietarySecurityIdentificationScheme>
	
	<owl:Class
		rdf:about="&fibo-sec-sec-id;FinancialInstrumentGlobalIdentifier">
		<rdfs:subClassOf
			rdf:resource="&fibo-fbc-fi-fi;FinancialInstrumentIdentifier"/>
		<rdfs:subClassOf
			rdf:resource="&fibo-fbc-fct-ra;RegistryIdentifier"/>
		<rdfs:subClassOf>
			<owl:Restriction>
				<owl:allValuesFrom
					rdf:resource="&fibo-sec-sec-id;FinancialInstrumentGlobalIdentifierRegistrationAuthority"/>
				<owl:onProperty
					rdf:resource="&fibo-fbc-fct-ra;isRegisteredBy"/>
			</owl:Restriction>
		</rdfs:subClassOf>
		<rdfs:subClassOf>
			<owl:Restriction>
				<owl:allValuesFrom
					rdf:resource="&fibo-sec-sec-id;FinancialInstrumentGlobalIdentifierRegistry"/>
				<owl:onProperty
					rdf:resource="&fibo-fbc-fct-ra;isRegisteredIn"/>
			</owl:Restriction>
		</rdfs:subClassOf>
		<rdfs:subClassOf>
			<owl:Restriction>
				<owl:allValuesFrom
					rdf:resource="&fibo-sec-sec-id;FinancialInstrumentGlobalIdentifierScheme"/>
				<owl:onProperty
					rdf:resource="&fibo-fnd-rel-rel;hasDefinition"/>
			</owl:Restriction>
		</rdfs:subClassOf>
		<rdfs:label>financial instrument global identifier</rdfs:label>
		<rdfs:isDefinedBy
			rdf:resource="http://www.omg.org/spec/FIGI/"/>
		<skos:definition>a financial instrument identifier that is defined as specified in the Object Management Group (OMG) Financial Instrument Global Identifier (FIGI) Specification</skos:definition>
		<fibo-fnd-utl-av:abbreviation>FIGI</fibo-fnd-utl-av:abbreviation>
	</owl:Class>
	
	<owl:Class
		rdf:about="&fibo-sec-sec-id;FinancialInstrumentGlobalIdentifierRegistrationAuthority">
		<rdfs:subClassOf
			rdf:resource="&fibo-fbc-fct-ra;RegistrationAuthority"/>
		<rdfs:subClassOf>
			<owl:Restriction>
				<owl:allValuesFrom
					rdf:resource="&fibo-sec-sec-id;FinancialInstrumentGlobalIdentifier"/>
				<owl:onProperty
					rdf:resource="&fibo-fbc-fct-rga;issues"/>
			</owl:Restriction>
		</rdfs:subClassOf>
		<rdfs:subClassOf>
			<owl:Restriction>
				<owl:hasValue
					rdf:resource="&fibo-sec-sec-id;BloombergLP"/>
				<owl:onProperty
					rdf:resource="&fibo-fnd-rel-rel;hasIdentity"/>
			</owl:Restriction>
		</rdfs:subClassOf>
		<rdfs:subClassOf>
			<owl:Restriction>
				<owl:onClass
					rdf:resource="&fibo-sec-sec-id;FinancialInstrumentGlobalIdentifierRegistry"/>
				<owl:onProperty
					rdf:resource="&fibo-fnd-rel-rel;manages"/>
				<owl:qualifiedCardinality
					rdf:datatype="&xsd;nonNegativeInteger">1</owl:qualifiedCardinality>
			</owl:Restriction>
		</rdfs:subClassOf>
		<rdfs:subClassOf>
			<owl:Restriction>
				<owl:onProperty
					rdf:resource="&fibo-fbc-fct-ra;registers"/>
				<owl:someValuesFrom
					rdf:resource="&fibo-sec-sec-id;FinancialInstrumentGlobalIdentifier"/>
			</owl:Restriction>
		</rdfs:subClassOf>
		<rdfs:label>Financial Instrument Global Identifier (FIGI) registration authority</rdfs:label>
		<rdfs:hasDefinition
			rdf:resource="http://www.omg.org/spec/FIGI/"/>
		<skos:definition>an internationally recognized registration authority for FIGIs</skos:definition>
		<fibo-fnd-utl-av:abbreviation>FIGI RA</fibo-fnd-utl-av:abbreviation>
	</owl:Class>
	
	<owl:Class
		rdf:about="&fibo-sec-sec-id;FinancialInstrumentGlobalIdentifierRegistry">
		<rdfs:subClassOf
			rdf:resource="&fibo-fbc-fct-ra;Registry"/>
		<rdfs:subClassOf>
			<owl:Restriction>
				<owl:allValuesFrom
					rdf:resource="&fibo-sec-sec-id;FinancialInstrumentGlobalIdentifierRegistryEntry"/>
				<owl:onProperty
					rdf:resource="&fibo-fbc-fct-ra;hasRegistryEntry"/>
			</owl:Restriction>
		</rdfs:subClassOf>
		<rdfs:subClassOf>
			<owl:Restriction>
				<owl:onClass
					rdf:resource="&fibo-sec-sec-id;FinancialInstrumentGlobalIdentifierRegistrationAuthority"/>
				<owl:onProperty
					rdf:resource="&fibo-fnd-rel-rel;isManagedBy"/>
				<owl:qualifiedCardinality
					rdf:datatype="&xsd;nonNegativeInteger">1</owl:qualifiedCardinality>
			</owl:Restriction>
		</rdfs:subClassOf>
		<rdfs:subClassOf>
			<owl:Restriction>
				<owl:onClass
					rdf:resource="&fibo-sec-sec-id;FinancialInstrumentGlobalIdentifierScheme"/>
				<owl:onProperty
					rdf:resource="&fibo-be-fct-fct;isCharacterizedBy"/>
				<owl:qualifiedCardinality
					rdf:datatype="&xsd;nonNegativeInteger">1</owl:qualifiedCardinality>
			</owl:Restriction>
		</rdfs:subClassOf>
		<rdfs:label>Financial Instrument Global Identifier (FIGI) Registry</rdfs:label>
		<rdfs:seeAlso
			rdf:resource="http://www.openfigi.com/"/>
		<skos:definition>an open, OMG standards-based registry used by the FIGI registration authority to manage the financial instrument identifiers and related information that it registers according to the Financial Instrument Global Identifier (FIGI) standard</skos:definition>
		<fibo-fnd-utl-av:abbreviation>FIGI Registry</fibo-fnd-utl-av:abbreviation>
	</owl:Class>
	
	<owl:Class
		rdf:about="&fibo-sec-sec-id;FinancialInstrumentGlobalIdentifierRegistryEntry">
		<rdfs:subClassOf
			rdf:resource="&fibo-fbc-fct-ra;RegistryEntry"/>
		<rdfs:subClassOf>
			<owl:Restriction>
				<owl:allValuesFrom
					rdf:resource="&fibo-fbc-fi-fi;FinancialInstrument"/>
				<owl:onProperty
					rdf:resource="&fibo-fnd-rel-rel;appliesTo"/>
			</owl:Restriction>
		</rdfs:subClassOf>
		<rdfs:subClassOf>
			<owl:Restriction>
				<owl:allValuesFrom
					rdf:resource="&fibo-sec-sec-id;FinancialInstrumentGlobalIdentifierRegistry"/>
				<owl:onProperty
					rdf:resource="&fibo-fbc-pas-fpas;isConstituentOf"/>
			</owl:Restriction>
		</rdfs:subClassOf>
		<rdfs:subClassOf>
			<owl:Restriction>
				<owl:onProperty
					rdf:resource="&fibo-fnd-rel-rel;comprises"/>
				<owl:someValuesFrom
					rdf:resource="&fibo-sec-sec-id;FinancialInstrumentGlobalIdentifier"/>
			</owl:Restriction>
		</rdfs:subClassOf>
		<rdfs:label>Financial Instrument Global Identifier (FIGI) registry entry</rdfs:label>
		<skos:definition>an entry in a Financial Instrument Global Identifier (FIGI) registry</skos:definition>
		<fibo-fnd-utl-av:abbreviation>FIGI registry entry</fibo-fnd-utl-av:abbreviation>
	</owl:Class>
	
	<owl:Class
		rdf:about="&fibo-sec-sec-id;FinancialInstrumentGlobalIdentifierScheme">
		<rdfs:subClassOf
			rdf:resource="&fibo-fbc-fct-ra;RegistrationScheme"/>
		<rdfs:subClassOf
			rdf:resource="&fibo-sec-sec-id;FinancialInstrumentIdentificationScheme"/>
		<rdfs:subClassOf>
			<owl:Restriction>
				<owl:allValuesFrom
					rdf:resource="&fibo-sec-sec-id;FinancialInstrumentGlobalIdentifier"/>
				<owl:onProperty
					rdf:resource="&fibo-fnd-rel-rel;defines"/>
			</owl:Restriction>
		</rdfs:subClassOf>
		<rdfs:subClassOf>
			<owl:Restriction>
				<owl:onProperty
					rdf:resource="&fibo-fnd-rel-rel;characterizes"/>
				<owl:someValuesFrom
					rdf:resource="&fibo-sec-sec-id;FinancialInstrumentGlobalIdentifierRegistry"/>
			</owl:Restriction>
		</rdfs:subClassOf>
		<rdfs:label>financial instrument global identifier scheme</rdfs:label>
		<rdfs:hasDefinition
			rdf:resource="http://www.omg.org/spec/FIGI/"/>
		<skos:definition>a standard identification scheme for financial instrument identifiers (not limited to securities) published by the Object Management Group (OMG)</skos:definition>
		<fibo-fnd-utl-av:abbreviation>FIGI scheme</fibo-fnd-utl-av:abbreviation>
	</owl:Class>
	
	<owl:Class
		rdf:about="&fibo-sec-sec-id;FinancialInstrumentIdentificationScheme">
		<rdfs:subClassOf
			rdf:resource="&fibo-fnd-arr-id;IdentificationScheme"/>
		<rdfs:subClassOf>
			<owl:Restriction>
				<owl:allValuesFrom
					rdf:resource="&fibo-fbc-fi-fi;FinancialInstrumentIdentifier"/>
				<owl:onProperty
					rdf:resource="&fibo-fnd-rel-rel;defines"/>
			</owl:Restriction>
		</rdfs:subClassOf>
		<rdfs:label>financial instrument identification scheme</rdfs:label>
		<skos:definition>a formal definition of the structure and application of a particular set of financial instrument identifiers</skos:definition>
	</owl:Class>
	
	<owl:Class
		rdf:about="&fibo-sec-sec-id;InternationalSecuritiesIdentificationNumber">
		<rdfs:subClassOf
			rdf:resource="&fibo-sec-sec-id;SecurityIdentifier"/>
		<rdfs:subClassOf>
			<owl:Restriction>
				<owl:allValuesFrom
					rdf:resource="&fibo-sec-sec-id;NationalSecuritiesIdentifyingNumber"/>
				<owl:onProperty
					rdf:resource="&fibo-fnd-rel-rel;hasPart"/>
			</owl:Restriction>
		</rdfs:subClassOf>
		<rdfs:label>international securities identification number</rdfs:label>
		<rdfs:seeAlso
			rdf:resource="http://www.iso.org/iso/catalogue_detail?csnumber=44811"/>
		<skos:definition>a security identifier that is defined as specified in ISO 6166, Securities and related financial instruments -- International securities identification numbering system (ISIN)</skos:definition>
		<fibo-fnd-utl-av:abbreviation>ISIN</fibo-fnd-utl-av:abbreviation>
	</owl:Class>
	
	<owl:Class
		rdf:about="&fibo-sec-sec-id;InternationalSecuritiesIdentificationNumberingScheme">
		<rdfs:subClassOf
			rdf:resource="&fibo-fbc-fct-ra;RegistrationScheme"/>
		<rdfs:subClassOf
			rdf:resource="&fibo-sec-sec-id;SecurityIdentificationScheme"/>
		<rdfs:subClassOf>
			<owl:Restriction>
				<owl:allValuesFrom
					rdf:resource="&fibo-sec-sec-id;InternationalSecuritiesIdentificationNumber"/>
				<owl:onProperty
					rdf:resource="&fibo-fnd-rel-rel;defines"/>
			</owl:Restriction>
		</rdfs:subClassOf>
		<rdfs:label>international securities identification numbering scheme</rdfs:label>
		<rdfs:seeAlso
			rdf:resource="http://www.iso.org/iso/catalogue_detail?csnumber=44811"/>
		<skos:definition>a formal definition of the structure and application of a ISINs as defined in ISO 6166</skos:definition>
		<fibo-fnd-utl-av:abbreviation>ISIN scheme</fibo-fnd-utl-av:abbreviation>
	</owl:Class>
	
	<owl:Class
		rdf:about="&fibo-sec-sec-id;ListedSecurityIdentifier">
		<rdfs:subClassOf
			rdf:resource="&fibo-sec-sec-id;SecurityIdentifier"/>
		<rdfs:subClassOf>
			<owl:Restriction>
				<owl:allValuesFrom
					rdf:resource="&fibo-sec-sec-id;ExchangeSpecificSecurityIdentificationScheme"/>
				<owl:onProperty
					rdf:resource="&fibo-fnd-rel-rel;hasDefinition"/>
			</owl:Restriction>
		</rdfs:subClassOf>
		<rdfs:subClassOf>
			<owl:Restriction>
				<owl:onClass
					rdf:resource="&fibo-sec-sec-lst;ListedSecurity"/>
				<owl:onProperty
					rdf:resource="&fibo-fnd-aap-agt;identifies"/>
				<owl:qualifiedCardinality
					rdf:datatype="&xsd;nonNegativeInteger">1</owl:qualifiedCardinality>
			</owl:Restriction>
		</rdfs:subClassOf>
		<rdfs:subClassOf>
			<owl:Restriction>
				<owl:onProperty
					rdf:resource="&fibo-fbc-fct-ra;isRegisteredBy"/>
				<owl:someValuesFrom
					rdf:resource="&fibo-sec-sec-lst;SecuritiesExchange"/>
			</owl:Restriction>
		</rdfs:subClassOf>
		<rdfs:subClassOf>
			<owl:Restriction>
				<owl:onProperty
					rdf:resource="&fibo-fbc-fct-ra;isRegisteredIn"/>
				<owl:someValuesFrom
					rdf:resource="&fibo-sec-sec-id;ExchangeSpecificSecuritiesRegistry"/>
			</owl:Restriction>
		</rdfs:subClassOf>
		<rdfs:label>listed security identifier</rdfs:label>
		<skos:definition>a security identifier issued in the public domain and referred to in listings and other relevant publications</skos:definition>
	</owl:Class>
	
	<owl:Class
		rdf:about="&fibo-sec-sec-id;LondonStockExchange">
		<rdfs:label>london stock exchange</rdfs:label>
	</owl:Class>
	
	<owl:Class
		rdf:about="&fibo-sec-sec-id;NationalNumberingAgency">
		<rdfs:subClassOf
			rdf:resource="&fibo-fbc-fct-ra;RegistrationAuthority"/>
		<rdfs:subClassOf>
			<owl:Restriction>
				<owl:allValuesFrom
					rdf:resource="&fibo-fnd-law-jur;Jurisdiction"/>
				<owl:onProperty
					rdf:resource="&fibo-be-ge-ge;hasJurisdiction"/>
			</owl:Restriction>
		</rdfs:subClassOf>
		<rdfs:subClassOf>
			<owl:Restriction>
				<owl:allValuesFrom
					rdf:resource="&fibo-sec-sec-id;NationalSecuritiesIdentifyingNumber"/>
				<owl:onProperty
					rdf:resource="&fibo-fbc-fct-ra;registers"/>
			</owl:Restriction>
		</rdfs:subClassOf>
		<rdfs:subClassOf>
			<owl:Restriction>
				<owl:allValuesFrom
					rdf:resource="&fibo-sec-sec-id;NationalSecuritiesIdentifyingNumber"/>
				<owl:onProperty
					rdf:resource="&fibo-fbc-fct-rga;issues"/>
			</owl:Restriction>
		</rdfs:subClassOf>
		<rdfs:subClassOf>
			<owl:Restriction>
				<owl:onClass
					rdf:resource="&fibo-sec-sec-id;NationalSecuritiesIdentifyingNumberRegistry"/>
				<owl:onProperty
					rdf:resource="&fibo-fnd-rel-rel;manages"/>
				<owl:qualifiedCardinality
					rdf:datatype="&xsd;nonNegativeInteger">1</owl:qualifiedCardinality>
			</owl:Restriction>
		</rdfs:subClassOf>
		<rdfs:label>national numbering agency</rdfs:label>
		<skos:definition>a registration authority responsible for issuing and managing National Securities Identifying Numbers for securities in accordance with the ISO 6166 standard in some jurisdiction (typically that of a country)</skos:definition>
		<fibo-fnd-utl-av:abbreviation>NNA</fibo-fnd-utl-av:abbreviation>
	</owl:Class>
	
	<owl:Class
		rdf:about="&fibo-sec-sec-id;NationalSecuritiesIdentifyingNumber">
		<rdfs:subClassOf
			rdf:resource="&fibo-sec-sec-id;SecurityIdentifier"/>
		<rdfs:subClassOf>
			<owl:Restriction>
				<owl:allValuesFrom
					rdf:resource="&fibo-sec-sec-id;InternationalSecuritiesIdentificationNumber"/>
				<owl:onProperty
					rdf:resource="&fibo-fnd-rel-rel;isPartOf"/>
			</owl:Restriction>
		</rdfs:subClassOf>
		<rdfs:subClassOf>
			<owl:Restriction>
				<owl:allValuesFrom
					rdf:resource="&fibo-sec-sec-id;NationalSecurityIdentificationScheme"/>
				<owl:onProperty
					rdf:resource="&fibo-fnd-rel-rel;hasDefinition"/>
			</owl:Restriction>
		</rdfs:subClassOf>
		<rdfs:subClassOf>
			<owl:Restriction>
				<owl:onClass
					rdf:resource="&fibo-fbc-fi-fi;Security"/>
				<owl:onProperty
					rdf:resource="&fibo-fnd-aap-agt;identifies"/>
				<owl:qualifiedCardinality
					rdf:datatype="&xsd;nonNegativeInteger">1</owl:qualifiedCardinality>
			</owl:Restriction>
		</rdfs:subClassOf>
		<rdfs:subClassOf>
			<owl:Restriction>
				<owl:onProperty
					rdf:resource="&fibo-fbc-fct-ra;isRegisteredBy"/>
				<owl:someValuesFrom
					rdf:resource="&fibo-sec-sec-id;NationalNumberingAgency"/>
			</owl:Restriction>
		</rdfs:subClassOf>
		<rdfs:label>National Securities Identifying Number</rdfs:label>
		<skos:definition>a generic, nine-digit alpha numeric code which identifies a fungible security, assigned by a national numbering agency under the ISO 6166 standard</skos:definition>
		<fibo-fnd-utl-av:abbreviation>NSIN</fibo-fnd-utl-av:abbreviation>
	</owl:Class>
	
	<owl:Class
		rdf:about="&fibo-sec-sec-id;NationalSecuritiesIdentifyingNumberRegistry">
		<rdfs:subClassOf
			rdf:resource="&fibo-fbc-fct-ra;Registry"/>
		<rdfs:subClassOf>
			<owl:Restriction>
				<owl:allValuesFrom
					rdf:resource="&fibo-sec-sec-id;NationalSecuritiesIdentifyingNumberRegistryEntry"/>
				<owl:onProperty
					rdf:resource="&fibo-fbc-fct-ra;hasRegistryEntry"/>
			</owl:Restriction>
		</rdfs:subClassOf>
		<rdfs:subClassOf>
			<owl:Restriction>
				<owl:onClass
					rdf:resource="&fibo-sec-sec-id;NationalNumberingAgency"/>
				<owl:onProperty
					rdf:resource="&fibo-fnd-rel-rel;isManagedBy"/>
				<owl:qualifiedCardinality
					rdf:datatype="&xsd;nonNegativeInteger">1</owl:qualifiedCardinality>
			</owl:Restriction>
		</rdfs:subClassOf>
		<rdfs:subClassOf>
			<owl:Restriction>
				<owl:onClass
					rdf:resource="&fibo-sec-sec-id;NationalSecurityIdentificationScheme"/>
				<owl:onProperty
					rdf:resource="&fibo-be-fct-fct;isCharacterizedBy"/>
				<owl:qualifiedCardinality
					rdf:datatype="&xsd;nonNegativeInteger">1</owl:qualifiedCardinality>
			</owl:Restriction>
		</rdfs:subClassOf>
		<rdfs:label>National Securities Identifying Number registry</rdfs:label>
		<skos:definition>a registry used by a national numbering agency to manage the financial instrument identifiers and related information that it registers</skos:definition>
		<fibo-fnd-utl-av:abbreviation>NSIN registry</fibo-fnd-utl-av:abbreviation>
	</owl:Class>
	
	<owl:Class
		rdf:about="&fibo-sec-sec-id;NationalSecuritiesIdentifyingNumberRegistryEntry">
		<rdfs:subClassOf
			rdf:resource="&fibo-fbc-fct-ra;RegistryEntry"/>
		<rdfs:subClassOf>
			<owl:Restriction>
				<owl:allValuesFrom
					rdf:resource="&fibo-fbc-fi-fi;Security"/>
				<owl:onProperty
					rdf:resource="&fibo-fnd-rel-rel;appliesTo"/>
			</owl:Restriction>
		</rdfs:subClassOf>
		<rdfs:subClassOf>
			<owl:Restriction>
				<owl:allValuesFrom
					rdf:resource="&fibo-sec-sec-id;NationalSecuritiesIdentifyingNumberRegistry"/>
				<owl:onProperty
					rdf:resource="&fibo-fbc-pas-fpas;isConstituentOf"/>
			</owl:Restriction>
		</rdfs:subClassOf>
		<rdfs:subClassOf>
			<owl:Restriction>
				<owl:onProperty
					rdf:resource="&fibo-fnd-rel-rel;comprises"/>
				<owl:someValuesFrom
					rdf:resource="&fibo-sec-sec-id;NationalSecuritiesIdentifyingNumber"/>
			</owl:Restriction>
		</rdfs:subClassOf>
		<rdfs:label>national numbering agency registry entry</rdfs:label>
		<skos:definition>an entry in a National Securities Identifying Number registry</skos:definition>
	</owl:Class>
	
	<owl:Class
		rdf:about="&fibo-sec-sec-id;NationalSecurityIdentificationScheme">
		<rdfs:subClassOf
			rdf:resource="&fibo-fbc-fct-ra;RegistrationScheme"/>
		<rdfs:subClassOf
			rdf:resource="&fibo-sec-sec-id;SecurityIdentificationScheme"/>
		<rdfs:subClassOf>
			<owl:Restriction>
				<owl:allValuesFrom
					rdf:resource="&fibo-sec-sec-id;NationalSecuritiesIdentifyingNumber"/>
				<owl:onProperty
					rdf:resource="&fibo-fnd-rel-rel;defines"/>
			</owl:Restriction>
		</rdfs:subClassOf>
		<rdfs:subClassOf>
			<owl:Restriction>
				<owl:allValuesFrom
					rdf:resource="&fibo-sec-sec-id;NationalSecuritiesIdentifyingNumberRegistry"/>
				<owl:onProperty
					rdf:resource="&fibo-fnd-rel-rel;characterizes"/>
			</owl:Restriction>
		</rdfs:subClassOf>
		<rdfs:subClassOf>
			<owl:Restriction>
				<owl:onProperty
					rdf:resource="&fibo-fnd-rel-rel;appliesTo"/>
				<owl:someValuesFrom
					rdf:resource="&fibo-fnd-law-jur;Jurisdiction"/>
			</owl:Restriction>
		</rdfs:subClassOf>
		<rdfs:label>national security identification scheme</rdfs:label>
		<skos:definition>a security identification scheme, defining the format and structure of a National Securities Identifying Number (NSIN), published nationally on behalf of a country</skos:definition>
		<fibo-fnd-utl-av:explanatoryNote>generally incorporated into the ISIN scheme as well</fibo-fnd-utl-av:explanatoryNote>
	</owl:Class>
	
	<owl:Class
		rdf:about="&fibo-sec-sec-id;ProprietarySecurityIdentificationScheme">
		<rdfs:subClassOf
			rdf:resource="&fibo-sec-sec-id;SecurityIdentificationScheme"/>
		<rdfs:subClassOf>
			<owl:Restriction>
				<owl:allValuesFrom
					rdf:resource="&fibo-sec-sec-id;ProprietarySecurityIdentifier"/>
				<owl:onProperty
					rdf:resource="&fibo-fnd-rel-rel;defines"/>
			</owl:Restriction>
		</rdfs:subClassOf>
		<rdfs:label>proprietary security identification scheme</rdfs:label>
		<skos:definition>a security identification scheme published by a data provider or other commercial entity</skos:definition>
	</owl:Class>
	
	<owl:Class
		rdf:about="&fibo-sec-sec-id;ProprietarySecurityIdentifier">
		<rdfs:subClassOf
			rdf:resource="&fibo-sec-sec-id;SecurityIdentifier"/>
		<rdfs:subClassOf>
			<owl:Restriction>
				<owl:allValuesFrom
					rdf:resource="&fibo-sec-sec-id;ProprietarySecurityIdentificationScheme"/>
				<owl:onProperty
					rdf:resource="&fibo-fnd-rel-rel;hasDefinition"/>
			</owl:Restriction>
		</rdfs:subClassOf>
		<rdfs:subClassOf>
			<owl:Restriction>
				<owl:onClass
					rdf:resource="&fibo-fbc-fi-fi;Security"/>
				<owl:onProperty
					rdf:resource="&fibo-fnd-aap-agt;identifies"/>
				<owl:qualifiedCardinality
					rdf:datatype="&xsd;nonNegativeInteger">1</owl:qualifiedCardinality>
			</owl:Restriction>
		</rdfs:subClassOf>
		<rdfs:label>proprietary security identifier</rdfs:label>
		<skos:definition>an identifier supplied by a commercial data provider or government, such as a RIC code</skos:definition>
	</owl:Class>
	
	<fibo-sec-sec-id:ProprietarySecurityIdentificationScheme
		rdf:about="&fibo-sec-sec-id;RICSScheme">
		<rdf:type
			rdf:resource="&owl;NamedIndividual"/>
	</fibo-sec-sec-id:ProprietarySecurityIdentificationScheme>
	
	<owl:Class
		rdf:about="&fibo-sec-sec-id;ReutersInstrumentCode">
		<rdfs:subClassOf
			rdf:resource="&fibo-sec-sec-id;ProprietarySecurityIdentifier"/>
		<rdfs:subClassOf>
			<owl:Restriction>
				<owl:hasValue
					rdf:resource="&fibo-sec-sec-id;ThomsonReuters"/>
				<owl:onProperty
					rdf:resource="&fibo-fbc-fct-rga;isIssuedBy"/>
			</owl:Restriction>
		</rdfs:subClassOf>
		<rdfs:label>Reuters instrument code</rdfs:label>
		<skos:definition>a ticker-like identifier to identify financial instruments and indices owned, managed, and distributed by Thomson Reuters</skos:definition>
		<fibo-fnd-utl-av:abbreviation>RIC</fibo-fnd-utl-av:abbreviation>
	</owl:Class>
	
	<rdf:Description
		rdf:about="&fibo-sec-sec-id;SEDOLMasterFile">
		<rdf:type
			rdf:resource="&owl;NamedIndividual"/>
		<rdf:type
			rdf:resource="&fibo-sec-sec-id;ExchangeSpecificSecuritiesRegistry"/>
		<rdf:type
			rdf:resource="&fibo-sec-sec-id;NationalSecuritiesIdentifyingNumberRegistry"/>
		<rdfs:label>SEDOL Master File</rdfs:label>
		<rdfs:seeAlso
			rdf:resource="http://www.londonstockexchange.com/products-and-services/reference-data/sedol-master-file/sedol-master-file.htm"/>
		<skos:definition>individual representing the SEDOL Master File, a repository of security identifiers, issued by the London Stock Exchange, that is the National Securities Identifying Number (NSIN) for securities issued in the United Kingdom, which is also part of the ISIN for the security it identifies</skos:definition>
		<fibo-fnd-rel-rel:isManagedBy
			rdf:resource="&fibo-sec-sec-id;LondonStockExchange"/>
	</rdf:Description>
	
	<fibo-be-plc-plc:PrivateCompanyWithLimitedLiability
		rdf:about="&fibo-sec-sec-id;SPGlobalMarketIntelligence">
		<rdf:type
			rdf:resource="&owl;NamedIndividual"/>
		<rdfs:label>S&amp;P Global Market Intelligence</rdfs:label>
		<rdfs:seeAlso
			rdf:resource="http://www.spcapitaliq.com/"/>
		<skos:definition>individual representing the S&amp;P Global Market Intelligence legal entity, a division of McGraw Hill Financial that is a global business and financial information services provider that also manages CUSIP Global Services</skos:definition>
		<fibo-fnd-rel-rel:hasLegalName>S&amp;P Global Market Intelligence</fibo-fnd-rel-rel:hasLegalName>
	</fibo-be-plc-plc:PrivateCompanyWithLimitedLiability>
	
	<owl:Class
		rdf:about="&fibo-sec-sec-id;SecurityIdentificationScheme">
		<rdfs:subClassOf
			rdf:resource="&fibo-sec-sec-id;FinancialInstrumentIdentificationScheme"/>
		<rdfs:subClassOf>
			<owl:Restriction>
				<owl:allValuesFrom
					rdf:resource="&fibo-sec-sec-id;SecurityIdentifier"/>
				<owl:onProperty
					rdf:resource="&fibo-fnd-rel-rel;defines"/>
			</owl:Restriction>
		</rdfs:subClassOf>
		<rdfs:label>security identification scheme</rdfs:label>
		<skos:definition>a formal definition of the structure and application of a particular set of securities identifiers</skos:definition>
	</owl:Class>
	
	<owl:Class
		rdf:about="&fibo-sec-sec-id;SecurityIdentifier">
		<rdfs:subClassOf
			rdf:resource="&fibo-fbc-fi-fi;FinancialInstrumentIdentifier"/>
		<rdfs:subClassOf>
			<owl:Restriction>
				<owl:onClass
					rdf:resource="&fibo-fbc-fi-fi;Security"/>
				<owl:onProperty
					rdf:resource="&fibo-fnd-aap-agt;identifies"/>
				<owl:qualifiedCardinality
					rdf:datatype="&xsd;nonNegativeInteger">1</owl:qualifiedCardinality>
			</owl:Restriction>
		</rdfs:subClassOf>
		<rdfs:subClassOf>
			<owl:Restriction>
				<owl:onClass
					rdf:resource="&fibo-sec-sec-id;SecurityIdentificationScheme"/>
				<owl:onProperty
					rdf:resource="&fibo-fnd-rel-rel;hasDefinition"/>
				<owl:qualifiedCardinality
					rdf:datatype="&xsd;nonNegativeInteger">1</owl:qualifiedCardinality>
			</owl:Restriction>
		</rdfs:subClassOf>
		<rdfs:label>security identifier</rdfs:label>
		<skos:definition>any publicly available identifier that is used to identify a security</skos:definition>
	</owl:Class>
	
	<owl:Class
		rdf:about="&fibo-sec-sec-id;StockExchangeDailyOfficialListCode">
		<rdfs:subClassOf
			rdf:resource="&fibo-sec-sec-id;ListedSecurityIdentifier"/>
		<rdfs:subClassOf
			rdf:resource="&fibo-sec-sec-id;NationalSecuritiesIdentifyingNumber"/>
		<rdfs:subClassOf
			rdf:resource="&fibo-sec-sec-id;ProprietarySecurityIdentifier"/>
		<rdfs:subClassOf>
			<owl:Restriction>
				<owl:hasValue
					rdf:resource="&fibo-sec-sec-id;LondonStockExchange"/>
				<owl:onProperty
					rdf:resource="&fibo-fbc-fct-ra;isRegisteredBy"/>
			</owl:Restriction>
		</rdfs:subClassOf>
		<rdfs:subClassOf>
			<owl:Restriction>
				<owl:hasValue
					rdf:resource="&fibo-sec-sec-id;SEDOLMasterFile"/>
				<owl:onProperty
					rdf:resource="&fibo-fbc-fct-ra;isRegisteredIn"/>
			</owl:Restriction>
		</rdfs:subClassOf>
		<rdfs:subClassOf>
			<owl:Restriction>
				<owl:hasValue
					rdf:resource="&fibo-sec-sec-id;StockExchangeDailyOfficialListScheme"/>
				<owl:onProperty
					rdf:resource="&fibo-fnd-rel-rel;hasDefinition"/>
			</owl:Restriction>
		</rdfs:subClassOf>
		<rdfs:label>Stock Exchange Daily Official List (SEDOL) code</rdfs:label>
		<rdfs:seeAlso
			rdf:resource="http://www.londonstockexchange.com/products-and-services/reference-data/sedol-master-file/sedol-master-file.htm"/>
		<rdfs:seeAlso
			rdf:resource="http://www.londonstockexchange.com/products-and-services/reference-data/sedol-master-file/sedolallocation.htm"/>
		<skos:definition>a seven character security identifier, issued by the London Stock Exchange, that is the National Securities Identifying Number (NSIN) for securities issued in the United Kingdom, which is also part of the ISIN for the security it identifies</skos:definition>
		<fibo-fnd-utl-av:abbreviation>SEDOL code</fibo-fnd-utl-av:abbreviation>
		<fibo-fnd-utl-av:adaptedFrom
			rdf:datatype="&xsd;anyURI">http://isin.net/?s=SEDOL</fibo-fnd-utl-av:adaptedFrom>
	</owl:Class>
	
	<rdf:Description
		rdf:about="&fibo-sec-sec-id;StockExchangeDailyOfficialListScheme">
		<rdf:type
			rdf:resource="&owl;NamedIndividual"/>
		<rdf:type
			rdf:resource="&fibo-sec-sec-id;ExchangeSpecificSecurityIdentificationScheme"/>
		<rdf:type
			rdf:resource="&fibo-sec-sec-id;NationalSecurityIdentificationScheme"/>
		<rdf:type
			rdf:resource="&fibo-sec-sec-id;ProprietarySecurityIdentificationScheme"/>
		<rdfs:label>Stock Exchange Daily Official List (SEDOL) scheme</rdfs:label>
		<rdfs:seeAlso
			rdf:resource="http://www.londonstockexchange.com/products-and-services/reference-data/sedol-master-file/sedolallocation.htm"/>
		<skos:definition>a national security idenfitifation scheme used to identify all stocks and registered bonds in the United Kingdom for the purposes of facilitating clearing and settlement of trades</skos:definition>
		<fibo-fnd-rel-rel:defines
			rdf:resource="&fibo-sec-sec-id;StockExchangeDailyOfficialListCode"/>
		<fibo-fnd-utl-av:abbreviation>SEDOL scheme</fibo-fnd-utl-av:abbreviation>
	</rdf:Description>
	
	<fibo-sec-sec-id:ProprietarySecurityIdentificationScheme
		rdf:about="&fibo-sec-sec-id;TelekursSecurityIDScheme">
		<rdf:type
			rdf:resource="&owl;NamedIndividual"/>
	</fibo-sec-sec-id:ProprietarySecurityIdentificationScheme>
	
	<owl:Class
		rdf:about="&fibo-sec-sec-id;ThomsonReuters">
		<rdfs:label>thomson reuters</rdfs:label>
	</owl:Class>
	
	<owl:ObjectProperty
		rdf:about="&fibo-sec-sec-id;hasNationalIdentifier">
		<rdfs:label>has national identifier</rdfs:label>
	</owl:ObjectProperty>

</rdf:RDF>