<?xml version="1.0" encoding="UTF-8"?>
  
<!DOCTYPE rdf:RDF [
    <!ENTITY fibo-ind-ind-val "http://spec.edmcouncil.org/fibo/red/ind/indicators/indicators-values/">
    <!ENTITY fibo-fnd-math-math "http://spec.edmcouncil.org/fibo/red/fnd/math/math/">
    <!ENTITY fibo-md-tmp-tmp "http://spec.edmcouncil.org/fibo/red/md/temporal-core/temporal-concepts/">
    <!ENTITY fibo-fnd-utl-bt "http://spec.edmcouncil.org/fibo/red/fnd/utilities/business-facing-types/">
    <!ENTITY fibo-fnd-tim-tim "http://spec.edmcouncil.org/fibo/red/fnd/date-time/date-time/">
]>

<rdf:RDF xmlns:xsd="http://www.w3.org/2001/XMLSchema#"
         xmlns:sm="http://www.omg.org/techprocess/ab/SpecificationMetadata/"
         xmlns:xs="http://www.w3.org/2001/XMLSchema"
         xmlns:fibo-fnd-utl-av="http://www.omg.org/spec/EDMC-FIBO/FND/Utilities/AnnotationVocabulary/"
         xmlns:rdf="http://www.w3.org/1999/02/22-rdf-syntax-ns#"
         xmlns:rdfs="http://www.w3.org/2000/01/rdf-schema#"
         xmlns:owl="http://www.w3.org/2002/07/owl#"
         xmlns:skos="http://www.w3.org/2004/02/skos/core#"
         xmlns:dc="http://purl.org/dc/terms/"
         xml:base="http://spec.edmcouncil.org/fibo/red/ind/indicators/indicators-values/">

   <owl:Ontology rdf:about="http://spec.edmcouncil.org/fibo/red/ind/indicators/indicators-values/">
      <owl:imports rdf:resource="http://spec.edmcouncil.org/fibo/red/fnd/math/math/"/>
      <owl:imports rdf:resource="http://spec.edmcouncil.org/fibo/red/md/temporal-core/temporal-concepts/"/>
      <owl:imports rdf:resource="http://spec.edmcouncil.org/fibo/red/fnd/utilities/business-facing-types/"/>
      <owl:imports rdf:resource="http://spec.edmcouncil.org/fibo/red/fnd/date-time/date-time/"/>
   </owl:Ontology>


  <!--
    ///////////////////////////////////////////////////////////////////////////////////////
    //
    // Datatypes
    //
    ///////////////////////////////////////////////////////////////////////////////////////
    -->



  <!--
    ///////////////////////////////////////////////////////////////////////////////////////
    //
    // Object Properties
    //
    ///////////////////////////////////////////////////////////////////////////////////////
    -->


<owl:ObjectProperty rdf:about="&fibo-ind-ind-val;forYear">
      <rdfs:label>for year</rdfs:label>
      <skos:definition>The year for which the GDP figure applies. Further Notes Review whether this needs additional qualifying terms, e.g. the applicable year end for that country.</skos:definition>
      <rdfs:domain rdf:resource="&fibo-ind-ind-val;GDPValue"/>
      <rdfs:range rdf:resource="&fibo-fnd-tim-tim;Year"/>
   </owl:ObjectProperty>

   <owl:ObjectProperty rdf:about="&fibo-ind-ind-val;hasGDPAmount">
      <rdfs:label>has g d p amount</rdfs:label>
      <skos:definition>The actual value of the GDP for the applicable period, stated as a monetary amount.</skos:definition>
      <rdfs:domain rdf:resource="&fibo-ind-ind-val;GDPValue"/>
      <rdfs:range rdf:resource="&fibo-md-tmp-tmp;DatedMonetaryAmount"/>
   </owl:ObjectProperty>

   <owl:ObjectProperty rdf:about="&fibo-ind-ind-val;measurementPeriod">
      <rdfs:label>measurement period</rdfs:label>
      <skos:definition>The period of time up to the quoted date, to which the inflation rate applies.</skos:definition>
      <rdfs:domain rdf:resource="&fibo-ind-ind-val;InflationRateValue"/>
      <rdfs:range rdf:resource="&fibo-fnd-tim-tim;Duration"/>
   </owl:ObjectProperty>

   <owl:ObjectProperty rdf:about="&fibo-ind-ind-val;applicablePeriod">
      <rdfs:label>applicable period</rdfs:label>
      <skos:definition>The period to which the stated value of the unemployment rate applies.</skos:definition>
      <rdfs:domain rdf:resource="&fibo-ind-ind-val;UnemploymentRateValue"/>
      <rdfs:range rdf:resource="&fibo-fnd-tim-tim;DatePeriod"/>
   </owl:ObjectProperty>


  <!--
    ///////////////////////////////////////////////////////////////////////////////////////
    //
    // Data Properties
    //
    ///////////////////////////////////////////////////////////////////////////////////////
    -->


<owl:DatatypeProperty rdf:about="&fibo-ind-ind-val;value">
      <rdfs:label>value</rdfs:label>
      <skos:definition>The exchange rate as a numerical ratio of the numerator to the denominator currency.</skos:definition>
      <rdfs:range rdf:resource="&fibo-fnd-utl-bt;number"/>
   </owl:DatatypeProperty>

   <owl:DatatypeProperty rdf:about="&fibo-ind-ind-val;hasPercentageValue">
      <rdfs:label>has percentage value</rdfs:label>
      <skos:definition>The actual value of the inflation rate, stated as a percentage.</skos:definition>
      <rdfs:range rdf:resource="&fibo-fnd-utl-bt;percentage"/>
   </owl:DatatypeProperty>

   <owl:DatatypeProperty rdf:about="&fibo-ind-ind-val;quotedDate">
      <rdfs:label>quoted date</rdfs:label>
      <skos:definition>The date to which the quoted inflation value applies.</skos:definition>
      <rdfs:range rdf:resource="http://www.w3.org/2001/XMLSchema#date"/>
   </owl:DatatypeProperty>

   <owl:DatatypeProperty rdf:about="&fibo-ind-ind-val;value.1">
      <rdfs:label>value</rdfs:label>
      <skos:definition>The quoted value of the Interest Rate at the specified time and date.</skos:definition>
      <rdfs:range rdf:resource="&fibo-fnd-utl-bt;percentage"/>
   </owl:DatatypeProperty>

   <owl:DatatypeProperty rdf:about="&fibo-ind-ind-val;value.2">
      <rdfs:label>value</rdfs:label>
      <skos:definition>The value of the benchmark as a number.</skos:definition>
      <rdfs:range rdf:resource="&fibo-fnd-utl-bt;wholeNumber"/>
   </owl:DatatypeProperty>

   <owl:DatatypeProperty rdf:about="&fibo-ind-ind-val;hasPercentageValue.1">
      <rdfs:label>has percentage value</rdfs:label>
      <skos:definition>The actual value of the unemployment rate, stated as a percentage of the population unemployed for the stated period.</skos:definition>
      <rdfs:range rdf:resource="&fibo-fnd-utl-bt;percentage"/>
   </owl:DatatypeProperty>


  <!--
    ///////////////////////////////////////////////////////////////////////////////////////
    //
    // Annotation Properties
    //
    ///////////////////////////////////////////////////////////////////////////////////////
    -->



  <!--
    ///////////////////////////////////////////////////////////////////////////////////////
    //
    // Classes
    //
    ///////////////////////////////////////////////////////////////////////////////////////
    -->


<owl:Class rdf:about="&fibo-ind-ind-val;EconomicRateQualifiedTimedValue">
      <rdfs:label>economic rate qualified timed value</rdfs:label>
      <rdfs:subClassOf rdf:resource="&fibo-ind-ind-val;MarketParameterTimedValue"/>
   </owl:Class>

   <owl:Class rdf:about="&fibo-ind-ind-val;ExchangeRateTimedValue">
      <rdfs:label>exchange rate timed value</rdfs:label>
   </owl:Class>

   <owl:Class rdf:about="&fibo-ind-ind-val;GDPValue">
      <rdfs:label>g d p value</rdfs:label>
      <rdfs:subClassOf rdf:resource="&fibo-ind-ind-val;EconomicRateQualifiedTimedValue"/>
   </owl:Class>

   <owl:Class rdf:about="&fibo-ind-ind-val;InflationRateValue">
      <rdfs:label>inflation rate value</rdfs:label>
      <skos:definition>The inflation rate, as a percentage. This is quoted for a period of time leading up to a specific date or month.</skos:definition>
   </owl:Class>

   <owl:Class rdf:about="&fibo-ind-ind-val;InterestRateTimedValue">
      <rdfs:label>interest rate timed value</rdfs:label>
      <skos:definition>The quoted value of the interest rate at the specified time and date. Term agreed; name changed from Interest Rate Value.</skos:definition>
   </owl:Class>

   <owl:Class rdf:about="&fibo-ind-ind-val;MarketParameterTimedValue">
      <rdfs:label>market parameter timed value</rdfs:label>
      <skos:definition>The actual value (at a point in time) of a parameter.</skos:definition>
      <rdfs:subClassOf rdf:resource="&fibo-fnd-math-math;TimedValue"/>
   </owl:Class>

   <owl:Class rdf:about="&fibo-ind-ind-val;ReferenceIndexDatedValue">
      <rdfs:label>reference index dated value</rdfs:label>
   </owl:Class>

   <owl:Class rdf:about="&fibo-ind-ind-val;UnemploymentRateValue">
      <rdfs:label>unemployment rate value</rdfs:label>
   </owl:Class>


  <!--
    ///////////////////////////////////////////////////////////////////////////////////////
    //
    // Individuals
    //
    ///////////////////////////////////////////////////////////////////////////////////////
    -->


</rdf:RDF>