<?xml version="1.0" encoding="UTF-8"?>
<rdf:RDF xmlns:xsd="http://www.w3.org/2001/XMLSchema#"
         xmlns:sm="http://www.omg.org/techprocess/ab/SpecificationMetadata/"
         xmlns:fibo-fnd-utl-av="http://www.omg.org/spec/EDMC-FIBO/FND/Utilities/AnnotationVocabulary/"
         xmlns:rdf="http://www.w3.org/1999/02/22-rdf-syntax-ns#"
         xmlns:rdfs="http://www.w3.org/2000/01/rdf-schema#"
         xmlns:owl="http://www.w3.org/2002/07/owl#"
         xmlns:skos="http://www.w3.org/2004/02/skos/core#"
         xmlns:dc="http://purl.org/dc/terms/"
         xml:base="http://www.edmcouncil.org/spec/EDMC-SR/BE/OwnershipAndControlExt/BERelations/">

   <owl:Ontology rdf:about="http://www.edmcouncil.org/spec/EDMC-SR/BE/OwnershipAndControlExt/BERelations/">
      <owl:imports rdf:resource="http://www.omg.org/spec/EDMC-SR/BE/OwnershipAndControl/CorporateControl/"/>
   </owl:Ontology>

   <!--Datatypes-->

<!--Object Properties-->

<owl:ObjectProperty rdf:about="http://www.edmcouncil.org/spec/EDMC-SR/BE/OwnershipAndControlExt/BERelations/constitutionallyPartOwnedBy">
      <skos:definition>Some entity which part owns the Formal Organization by means of some formal instrument such as shares or stockholder equity.</skos:definition>
      <rdfs:subPropertyOf rdf:resource="http://www.edmcouncil.org/spec/EDMC-SR/BE/OwnershipAndControlExt/BERelations/partOwnedBy"/>
      <rdfs:domain rdf:resource="http://www.omg.org/spec/EDMC-SR/BE/LegalEntities/FormalBusinessOrganizations/FormallyConstitutedOrganization"/>
      <rdfs:range rdf:resource="http://www.omg.org/spec/EDMC-SR/FND/Parties/Parties/IndependentParty"/>
   </owl:ObjectProperty>

   <owl:ObjectProperty rdf:about="http://www.edmcouncil.org/spec/EDMC-SR/BE/OwnershipAndControlExt/BERelations/controlledBy">
      <skos:definition>Some entity which controls the Formal Organization, this being some kind of autonomous agent.</skos:definition>
      <skos:editorialNote>This relationship corresponds to the party relation "Entity controlled by" and the scope of that party, by inheritance from "Party" itself, as being any Autonomous Agent. That is, any type of autonomous agent may be found in the role of the controlling party of some Formal Organization (this is the most general level of any type of control; types of de jure control may only be exerted by narrower ranges of types of entity).</skos:editorialNote>
      <rdfs:domain rdf:resource="http://www.omg.org/spec/EDMC-SR/BE/LegalEntities/FormalBusinessOrganizations/FormallyConstitutedOrganization"/>
      <rdfs:range rdf:resource="http://www.omg.org/spec/EDMC-SR/FND/AgentsAndPeople/Agents/AutonomousAgent"/>
   </owl:ObjectProperty>

   <owl:ObjectProperty rdf:about="http://www.edmcouncil.org/spec/EDMC-SR/BE/OwnershipAndControlExt/BERelations/hasLegalControlOf">
      <skos:definition>The entity has legal control over this organization.</skos:definition>
      <rdfs:domain rdf:resource="http://www.omg.org/spec/EDMC-SR/FND/Parties/Parties/IndependentParty"/>
      <rdfs:range rdf:resource="http://www.omg.org/spec/EDMC-SR/BE/LegalEntities/FormalBusinessOrganizations/FormallyConstitutedOrganization"/>
   </owl:ObjectProperty>

   <owl:ObjectProperty rdf:about="http://www.edmcouncil.org/spec/EDMC-SR/BE/OwnershipAndControlExt/BERelations/hasShareholder">
      <skos:definition>Some entity which part owns the Incorporated Company by means of shares.</skos:definition>
      <rdfs:subPropertyOf rdf:resource="http://www.edmcouncil.org/spec/EDMC-SR/BE/OwnershipAndControlExt/BERelations/constitutionallyPartOwnedBy"/>
      <rdfs:domain rdf:resource="http://www.omg.org/spec/EDMC-SR/BE/Corporations/Corporations/IncorporatedCompany"/>
      <rdfs:range rdf:resource="http://www.omg.org/spec/EDMC-SR/FND/Parties/Parties/IndependentParty"/>
   </owl:ObjectProperty>

   <owl:ObjectProperty rdf:about="http://www.edmcouncil.org/spec/EDMC-SR/BE/OwnershipAndControlExt/BERelations/hasShareholderFormalOrganization">
      <skos:definition>Some Formal Organization which part owns the Incorporated Company by means of shares.</skos:definition>
      <rdfs:subPropertyOf rdf:resource="http://www.edmcouncil.org/spec/EDMC-SR/BE/OwnershipAndControlExt/BERelations/hasShareholder"/>
      <rdfs:domain rdf:resource="http://www.omg.org/spec/EDMC-SR/BE/Corporations/Corporations/IncorporatedCompany"/>
      <rdfs:range rdf:resource="http://www.omg.org/spec/EDMC-SR/BE/LegalEntities/FormalBusinessOrganizations/FormallyConstitutedOrganization"/>
   </owl:ObjectProperty>

   <owl:ObjectProperty rdf:about="http://www.edmcouncil.org/spec/EDMC-SR/BE/OwnershipAndControlExt/BERelations/legallyControlledBy">
      <rdfs:subPropertyOf rdf:resource="http://www.edmcouncil.org/spec/EDMC-SR/BE/OwnershipAndControlExt/BERelations/controlledBy"/>
      <rdfs:domain rdf:resource="http://www.omg.org/spec/EDMC-SR/BE/LegalEntities/FormalBusinessOrganizations/FormallyConstitutedOrganization"/>
      <rdfs:range rdf:resource="http://www.omg.org/spec/EDMC-SR/FND/Parties/Parties/IndependentParty"/>
      <owl:inverseOf rdf:resource="http://www.edmcouncil.org/spec/EDMC-SR/BE/OwnershipAndControlExt/BERelations/hasLegalControlOf"/>
   </owl:ObjectProperty>

   <owl:ObjectProperty rdf:about="http://www.edmcouncil.org/spec/EDMC-SR/BE/OwnershipAndControlExt/BERelations/majorityControllingInterestBy">
      <skos:definition>Entity having controlling ownership of the Formal Organization.</skos:definition>
      <skos:editorialNote>This is defined as being anything above fifty percent of the controlling ownership, for example voting shares or contractually defined control percentages.</skos:editorialNote>
      <rdfs:domain rdf:resource="http://www.omg.org/spec/EDMC-SR/BE/LegalEntities/FormalBusinessOrganizations/FormallyConstitutedOrganization"/>
      <rdfs:range rdf:resource="http://www.omg.org/spec/EDMC-SR/FND/Parties/Parties/IndependentParty"/>
   </owl:ObjectProperty>

   <owl:ObjectProperty rdf:about="http://www.edmcouncil.org/spec/EDMC-SR/BE/OwnershipAndControlExt/BERelations/majorityControllingOwnershipBy">
      <skos:definition>Incorporated Company holding over fifty percent of the voting shares in this Incorporated Company.</skos:definition>
      <rdfs:subPropertyOf rdf:resource="http://www.edmcouncil.org/spec/EDMC-SR/BE/OwnershipAndControlExt/BERelations/someControllingInterestByCompany"/>
      <rdfs:domain rdf:resource="http://www.omg.org/spec/EDMC-SR/BE/Corporations/Corporations/IncorporatedCompany"/>
      <rdfs:range rdf:resource="http://www.omg.org/spec/EDMC-SR/BE/Corporations/Corporations/IncorporatedCompany"/>
   </owl:ObjectProperty>

   <owl:ObjectProperty rdf:about="http://www.edmcouncil.org/spec/EDMC-SR/BE/OwnershipAndControlExt/BERelations/majorityVotingShareholdingBy">
      <skos:definition>Formal Organization holding over fifty percent of the voting shares in this Incorporated Company.</skos:definition>
      <rdfs:subPropertyOf rdf:resource="http://www.edmcouncil.org/spec/EDMC-SR/BE/OwnershipAndControlExt/BERelations/majorityControllingInterestBy"/>
      <rdfs:subPropertyOf rdf:resource="http://www.edmcouncil.org/spec/EDMC-SR/BE/OwnershipAndControlExt/BERelations/someVotingShareholdingBy"/>
      <rdfs:domain rdf:resource="http://www.omg.org/spec/EDMC-SR/BE/Corporations/Corporations/IncorporatedCompany"/>
      <rdfs:range rdf:resource="http://www.omg.org/spec/EDMC-SR/BE/LegalEntities/FormalBusinessOrganizations/FormallyConstitutedOrganization"/>
   </owl:ObjectProperty>

   <owl:ObjectProperty rdf:about="http://www.edmcouncil.org/spec/EDMC-SR/BE/OwnershipAndControlExt/BERelations/partOwnedBy">
      <skos:definition>The entity is owned in some part by this kind of entity.</skos:definition>
      <skos:editorialNote>This relationship corresponds to the party "Entity Owning Party", which is defined as owning any Formal Organization, and being itself some potential owning party, that is the union of Formal Organization, Legal Person and legitimate organization.</skos:editorialNote>
      <rdfs:domain rdf:resource="http://www.omg.org/spec/EDMC-SR/BE/LegalEntities/FormalBusinessOrganizations/FormallyConstitutedOrganization"/>
      <rdfs:range rdf:resource="http://www.omg.org/spec/EDMC-SR/FND/Parties/Parties/IndependentParty"/>
   </owl:ObjectProperty>

   <owl:ObjectProperty rdf:about="http://www.edmcouncil.org/spec/EDMC-SR/BE/OwnershipAndControlExt/BERelations/significantControllingInterestBy">
      <skos:definition>Entity which has significant control of the Formal Organization.</skos:definition>
      <skos:editorialNote>This is defined as anything above a minimum threshold which is considered significant, but up to or below 50%.</skos:editorialNote>
      <rdfs:domain rdf:resource="http://www.omg.org/spec/EDMC-SR/BE/LegalEntities/FormalBusinessOrganizations/FormallyConstitutedOrganization"/>
      <rdfs:range rdf:resource="http://www.omg.org/spec/EDMC-SR/FND/Parties/Parties/IndependentParty"/>
   </owl:ObjectProperty>

   <owl:ObjectProperty rdf:about="http://www.edmcouncil.org/spec/EDMC-SR/BE/OwnershipAndControlExt/BERelations/significantControllingInterestByCompany">
      <skos:definition>Incorporated Company having a significant voting ownership in the Incorporated Company.</skos:definition>
      <rdfs:subPropertyOf rdf:resource="http://www.edmcouncil.org/spec/EDMC-SR/BE/OwnershipAndControlExt/BERelations/someControllingInterestByCompany"/>
      <rdfs:subPropertyOf rdf:resource="http://www.edmcouncil.org/spec/EDMC-SR/BE/OwnershipAndControlExt/BERelations/significantVotingShareholdingBy"/>
      <rdfs:domain rdf:resource="http://www.omg.org/spec/EDMC-SR/BE/Corporations/Corporations/IncorporatedCompany"/>
      <rdfs:range rdf:resource="http://www.omg.org/spec/EDMC-SR/BE/Corporations/Corporations/IncorporatedCompany"/>
   </owl:ObjectProperty>

   <owl:ObjectProperty rdf:about="http://www.edmcouncil.org/spec/EDMC-SR/BE/OwnershipAndControlExt/BERelations/significantVotingShareholdingBy">
      <skos:definition>Formal Organization having significant voting ownership in the Incorporated Company.</skos:definition>
      <rdfs:subPropertyOf rdf:resource="http://www.edmcouncil.org/spec/EDMC-SR/BE/OwnershipAndControlExt/BERelations/someVotingShareholdingBy"/>
      <rdfs:subPropertyOf rdf:resource="http://www.edmcouncil.org/spec/EDMC-SR/BE/OwnershipAndControlExt/BERelations/significantControllingInterestBy"/>
      <rdfs:domain rdf:resource="http://www.omg.org/spec/EDMC-SR/BE/Corporations/Corporations/IncorporatedCompany"/>
      <rdfs:range rdf:resource="http://www.omg.org/spec/EDMC-SR/BE/LegalEntities/FormalBusinessOrganizations/FormallyConstitutedOrganization"/>
   </owl:ObjectProperty>

   <owl:ObjectProperty rdf:about="http://www.edmcouncil.org/spec/EDMC-SR/BE/OwnershipAndControlExt/BERelations/someControllingInterestByCompany">
      <skos:definition>Company having some degree of voting ownership in the company.</skos:definition>
      <rdfs:subPropertyOf rdf:resource="http://www.edmcouncil.org/spec/EDMC-SR/BE/OwnershipAndControlExt/BERelations/someVotingShareholdingBy"/>
      <rdfs:domain rdf:resource="http://www.omg.org/spec/EDMC-SR/BE/Corporations/Corporations/IncorporatedCompany"/>
      <rdfs:range rdf:resource="http://www.omg.org/spec/EDMC-SR/BE/Corporations/Corporations/IncorporatedCompany"/>
   </owl:ObjectProperty>

   <owl:ObjectProperty rdf:about="http://www.edmcouncil.org/spec/EDMC-SR/BE/OwnershipAndControlExt/BERelations/someVotingShareholdingBy">
      <skos:definition>Formal Organization having some degree of voting ownership in the company.</skos:definition>
      <rdfs:domain rdf:resource="http://www.omg.org/spec/EDMC-SR/BE/Corporations/Corporations/IncorporatedCompany"/>
      <rdfs:range rdf:resource="http://www.omg.org/spec/EDMC-SR/BE/LegalEntities/FormalBusinessOrganizations/FormallyConstitutedOrganization"/>
   </owl:ObjectProperty>

   <owl:ObjectProperty rdf:about="http://www.edmcouncil.org/spec/EDMC-SR/BE/OwnershipAndControlExt/BERelations/totalVotingShareholdingBy">
      <skos:definition>Formal Organization holding all of the voting shares in the Incorporated Company.</skos:definition>
      <rdfs:subPropertyOf rdf:resource="http://www.edmcouncil.org/spec/EDMC-SR/BE/OwnershipAndControlExt/BERelations/majorityVotingShareholdingBy"/>
      <rdfs:domain rdf:resource="http://www.omg.org/spec/EDMC-SR/BE/Corporations/Corporations/IncorporatedCompany"/>
      <rdfs:range rdf:resource="http://www.omg.org/spec/EDMC-SR/BE/LegalEntities/FormalBusinessOrganizations/FormallyConstitutedOrganization"/>
   </owl:ObjectProperty>

   <owl:ObjectProperty rdf:about="http://www.edmcouncil.org/spec/EDMC-SR/BE/OwnershipAndControlExt/BERelations/whollyControlledBy">
      <skos:definition>Entity having controlling ownership of the Formal Organization.</skos:definition>
      <skos:editorialNote>This is defined as having 100% ownership (and therefore control ownership) of the formal Organization by whatever means is in place for ownership in that organization.</skos:editorialNote>
      <rdfs:subPropertyOf rdf:resource="http://www.edmcouncil.org/spec/EDMC-SR/BE/OwnershipAndControlExt/BERelations/legallyControlledBy"/>
      <rdfs:domain rdf:resource="http://www.omg.org/spec/EDMC-SR/BE/LegalEntities/FormalBusinessOrganizations/FormallyConstitutedOrganization"/>
      <rdfs:range rdf:resource="http://www.omg.org/spec/EDMC-SR/FND/Parties/Parties/IndependentParty"/>
   </owl:ObjectProperty>

   <owl:ObjectProperty rdf:about="http://www.edmcouncil.org/spec/EDMC-SR/BE/OwnershipAndControlExt/BERelations/whollyOwnedBy">
      <skos:definition>Incorporated Company holding all of the voting shares in the Incorporated Company.</skos:definition>
      <rdfs:subPropertyOf rdf:resource="http://www.edmcouncil.org/spec/EDMC-SR/BE/OwnershipAndControlExt/BERelations/totalVotingShareholdingBy"/>
      <rdfs:subPropertyOf rdf:resource="http://www.edmcouncil.org/spec/EDMC-SR/BE/OwnershipAndControlExt/BERelations/majorityControllingOwnershipBy"/>
      <rdfs:domain rdf:resource="http://www.omg.org/spec/EDMC-SR/BE/Corporations/Corporations/IncorporatedCompany"/>
      <rdfs:range rdf:resource="http://www.omg.org/spec/EDMC-SR/BE/Corporations/Corporations/IncorporatedCompany"/>
   </owl:ObjectProperty>

   <!--Data Properties-->

<!--Annotation Properties-->

<!--Classes-->

<!--Individuals-->

</rdf:RDF>