<?xml version="1.0" encoding="UTF-8"?>
<rdf:RDF xmlns:xsd="http://www.w3.org/2001/XMLSchema#"
         xmlns:sm="http://www.omg.org/techprocess/ab/SpecificationMetadata/"
         xmlns:fibo-fnd-utl-av="http://www.omg.org/spec/EDMC-FIBO/FND/Utilities/AnnotationVocabulary/"
         xmlns:rdf="http://www.w3.org/1999/02/22-rdf-syntax-ns#"
         xmlns:rdfs="http://www.w3.org/2000/01/rdf-schema#"
         xmlns:owl="http://www.w3.org/2002/07/owl#"
         xmlns:skos="http://www.w3.org/2004/02/skos/core#"
         xmlns:dc="http://purl.org/dc/terms/"
         xml:base="http://www.omg.org/spec/EDMC-SR/BE/LegalEntities/FormalBusinessOrganizations/">

   <owl:Ontology rdf:about="http://www.omg.org/spec/EDMC-SR/BE/LegalEntities/FormalBusinessOrganizations/">
      <owl:imports rdf:resource="http://www.omg.org/spec/EDMC-SR/FND/Organizations/FormalOrganizations/"/>
      <owl:imports rdf:resource="http://www.edmcouncil.org/spec/EDMC-SR/FND/Information/Identifiers/"/>
      <owl:imports rdf:resource="http://www.omg.org/spec/EDMC-SR/FND/Agreements/Contracts/"/>
   </owl:Ontology>

   <!--Datatypes-->

<!--Object Properties-->

<owl:ObjectProperty rdf:about="http://www.omg.org/spec/EDMC-SR/BE/LegalEntities/FormalBusinessOrganizations/formalBusinessOrganizationIsMemberOf">
      <rdfs:subPropertyOf rdf:resource="http://www.omg.org/spec/EDMC-SR/FND/Paties/Roles/hasRole"/>
      <rdfs:subPropertyOf rdf:resource="http://www.omg.org/spec/EDMC-SR/FND/Relations/Relations/isMemberOf"/>
      <rdfs:domain rdf:resource="http://www.omg.org/spec/EDMC-SR/BE/LegalEntities/FormalBusinessOrganizations/FormalBusinessOrganizationMember"/>
      <rdfs:range rdf:resource="http://www.omg.org/spec/EDMC-SR/BE/LegalEntities/FormalBusinessOrganizations/FormallyConstitutedOrganization"/>
   </owl:ObjectProperty>

   <owl:ObjectProperty rdf:about="http://www.omg.org/spec/EDMC-SR/BE/LegalEntities/FormalBusinessOrganizations/hasSectorClassification">
      <rdfs:subPropertyOf rdf:resource="http://www.omg.org/spec/EDMC-SR/FND/Relations/Relations/isClassifiedBy"/>
      <rdfs:domain rdf:resource="http://www.omg.org/spec/EDMC-SR/BE/LegalEntities/FormalBusinessOrganizations/FormallyConstitutedOrganization"/>
      <rdfs:range rdf:resource="http://www.omg.org/spec/EDMC-SR/BE/LegalEntities/FormalBusinessOrganizations/OrganizationIndustrySectorClassification"/>
      <owl:inverseOf rdf:resource="http://www.omg.org/spec/EDMC-SR/BE/LegalEntities/FormalBusinessOrganizations/organizatonIndustrySectorClassificaitonClassifies"/>
   </owl:ObjectProperty>

   <owl:ObjectProperty rdf:about="http://www.omg.org/spec/EDMC-SR/BE/LegalEntities/FormalBusinessOrganizations/formallyConstitutedOrganizationIsGovernedBy">
      <skos:definition>The or any agreement which governs the relationships among the principals in some formal organization.</skos:definition>
      <rdfs:subPropertyOf rdf:resource="http://www.omg.org/spec/EDMC-SR/FND/Relations/Relations/isGoverneBy"/>
      <rdfs:domain rdf:resource="http://www.omg.org/spec/EDMC-SR/BE/LegalEntities/FormalBusinessOrganizations/FormallyConstitutedOrganization"/>
      <rdfs:range rdf:resource="http://www.omg.org/spec/EDMC-SR/BE/LegalEntities/FormalBusinessOrganizations/OrganizationCoveringAgreement"/>
   </owl:ObjectProperty>

   <owl:ObjectProperty rdf:about="http://www.omg.org/spec/EDMC-SR/BE/LegalEntities/FormalBusinessOrganizations/formallyConstitutedOrganizationIsIdentifiedBy">
      <skos:definition>A formal, published identifier of the business entity.</skos:definition>
      <rdfs:subPropertyOf rdf:resource="http://www.omg.org/spec/EDMC-SR/FND/Relations/Relations/isIdentifiedBy"/>
      <rdfs:subPropertyOf rdf:resource="http://www.edmcouncil.org/spec/EDMC-SR/FND/Information/Identifiers/hasIdentifier"/>
      <rdfs:domain rdf:resource="http://www.omg.org/spec/EDMC-SR/BE/LegalEntities/FormalBusinessOrganizations/FormallyConstitutedOrganization"/>
      <rdfs:range rdf:resource="http://www.omg.org/spec/EDMC-SR/BE/LegalEntities/FormalBusinessOrganizations/OrganizationIdentificationCode"/>
   </owl:ObjectProperty>

   <owl:ObjectProperty rdf:about="http://www.omg.org/spec/EDMC-SR/BE/LegalEntities/FormalBusinessOrganizations/defines">
      <skos:definition>An organization identification code defined in the scheme.</skos:definition>
      <rdfs:subPropertyOf rdf:resource="http://www.edmcouncil.org/spec/EDMC-SR/FND/Information/Identifiers/defines"/>
      <rdfs:subPropertyOf rdf:resource="http://www.omg.org/spec/EDMC-SR/FND/Relations/Relations/defines"/>
      <rdfs:domain rdf:resource="http://www.omg.org/spec/EDMC-SR/BE/LegalEntities/FormalBusinessOrganizations/OrganizationIdentificationScheme"/>
      <rdfs:range rdf:resource="http://www.omg.org/spec/EDMC-SR/BE/LegalEntities/FormalBusinessOrganizations/OrganizationIdentificationCode"/>
   </owl:ObjectProperty>

   <owl:ObjectProperty rdf:about="http://www.omg.org/spec/EDMC-SR/BE/LegalEntities/FormalBusinessOrganizations/organizatonIndustrySectorClassificaitonClassifies">
      <skos:definition>A business entity which is covered by the classification.</skos:definition>
      <rdfs:subPropertyOf rdf:resource="http://www.edmcouncil.org/spec/EDMC-SR/FND/Information/Schemes/classifies"/>
      <rdfs:subPropertyOf rdf:resource="http://www.omg.org/spec/EDMC-SR/FND/Relations/Relations/classifies"/>
      <rdfs:domain rdf:resource="http://www.omg.org/spec/EDMC-SR/BE/LegalEntities/FormalBusinessOrganizations/OrganizationIndustrySectorClassification"/>
      <rdfs:range rdf:resource="http://www.omg.org/spec/EDMC-SR/BE/LegalEntities/FormalBusinessOrganizations/FormallyConstitutedOrganization"/>
   </owl:ObjectProperty>

   <owl:ObjectProperty rdf:about="http://www.omg.org/spec/EDMC-SR/BE/LegalEntities/FormalBusinessOrganizations/hasInternalEntity">
      <skos:definition>The organization has some part which is formally defined as an Internal Entity, for example for reporting, management or accounting purposes.</skos:definition>
      <rdfs:subPropertyOf rdf:resource="http://www.omg.org/spec/EDMC-SR/BE/LegalEntities/FormalBusinessOrganizations/hasSubUnit"/>
      <rdfs:domain rdf:resource="http://www.omg.org/spec/EDMC-SR/BE/LegalEntities/FormalBusinessOrganizations/FormallyConstitutedOrganization"/>
      <rdfs:range rdf:resource="http://www.omg.org/spec/EDMC-SR/BE/LegalEntities/FormalBusinessOrganizations/OrganizationalSubUnit"/>
   </owl:ObjectProperty>

   <owl:ObjectProperty rdf:about="http://www.omg.org/spec/EDMC-SR/BE/LegalEntities/FormalBusinessOrganizations/hasSubUnit">
      <rdfs:subPropertyOf rdf:resource="http://www.omg.org/spec/EDMC-SR/FND/Relations/Relations/hasPart"/>
      <rdfs:domain rdf:resource="http://www.omg.org/spec/EDMC-SR/BE/LegalEntities/FormalBusinessOrganizations/FormallyConstitutedOrganization"/>
      <rdfs:range rdf:resource="http://www.omg.org/spec/EDMC-SR/BE/LegalEntities/FormalBusinessOrganizations/OrganizationalSubUnit"/>
      <owl:inverseOf rdf:resource="http://www.omg.org/spec/EDMC-SR/BE/LegalEntities/FormalBusinessOrganizations/isSubUnitOf"/>
   </owl:ObjectProperty>

   <owl:ObjectProperty rdf:about="http://www.omg.org/spec/EDMC-SR/BE/LegalEntities/FormalBusinessOrganizations/hasEquity">
      <skos:definition>The Formal Organization has some form of Stockholder Equity.</skos:definition>
      <rdfs:domain rdf:resource="http://www.omg.org/spec/EDMC-SR/BE/LegalEntities/FormalBusinessOrganizations/FormallyConstitutedOrganization"/>
      <rdfs:range rdf:resource="http://www.omg.org/spec/EDMC-SR/FND/Accounting/AccountingEquity/StockholdersEquity"/>
   </owl:ObjectProperty>

   <owl:ObjectProperty rdf:about="http://www.omg.org/spec/EDMC-SR/BE/LegalEntities/FormalBusinessOrganizations/hasOperatingAddress">
      <skos:definition>Address at which the organization carries out its operations.</skos:definition>
      <rdfs:subPropertyOf rdf:resource="http://www.omg.org/spec/EDMC-SR/FND/Organizations/Organizations/organizationHasAddress"/>
      <rdfs:domain rdf:resource="http://www.omg.org/spec/EDMC-SR/BE/LegalEntities/FormalBusinessOrganizations/FormallyConstitutedOrganization"/>
      <rdfs:range rdf:resource="http://www.omg.org/spec/EDMC-SR/FND/Places/Addresses/PostalAddress"/>
   </owl:ObjectProperty>

   <owl:ObjectProperty rdf:about="http://www.omg.org/spec/EDMC-SR/BE/LegalEntities/FormalBusinessOrganizations/hasPrimaryAddress">
      <skos:definition>The main address at which communications to the organization may be addressed; its headquarters address.</skos:definition>
      <rdfs:subPropertyOf rdf:resource="http://www.omg.org/spec/EDMC-SR/FND/Organizations/Organizations/organizationHasAddress"/>
      <rdfs:domain rdf:resource="http://www.omg.org/spec/EDMC-SR/BE/LegalEntities/FormalBusinessOrganizations/FormallyConstitutedOrganization"/>
      <rdfs:range rdf:resource="http://www.omg.org/spec/EDMC-SR/FND/Places/Addresses/PostalAddress"/>
   </owl:ObjectProperty>

   <owl:ObjectProperty rdf:about="http://www.omg.org/spec/EDMC-SR/BE/LegalEntities/FormalBusinessOrganizations/hasRegisteredAddress">
      <skos:definition>The organization has an address at which it is registered and at which legal papers may be served on it.</skos:definition>
      <rdfs:subPropertyOf rdf:resource="http://www.omg.org/spec/EDMC-SR/FND/Organizations/Organizations/organizationHasAddress"/>
      <rdfs:domain rdf:resource="http://www.omg.org/spec/EDMC-SR/BE/LegalEntities/FormalBusinessOrganizations/FormallyConstitutedOrganization"/>
      <rdfs:range rdf:resource="http://www.omg.org/spec/EDMC-SR/BE/LegalEntities/FormalBusinessOrganizations/RegisteredAddress"/>
   </owl:ObjectProperty>

   <owl:ObjectProperty rdf:about="http://www.omg.org/spec/EDMC-SR/BE/LegalEntities/FormalBusinessOrganizations/hasSignatory">
      <skos:definition>has a party which is authorized to sign contracts on the party of the entity.</skos:definition>
      <rdfs:subPropertyOf rdf:resource="http://www.omg.org/spec/EDMC-SR/FND/Parties/Parties/hasPartyInRole"/>
      <rdfs:domain rdf:resource="http://www.omg.org/spec/EDMC-SR/BE/LegalEntities/FormalBusinessOrganizations/FormallyConstitutedOrganization"/>
      <rdfs:range rdf:resource="http://www.omg.org/spec/EDMC-SR/BE/LegalEntities/LegalPersons/Signatory"/>
   </owl:ObjectProperty>

   <owl:ObjectProperty rdf:about="http://www.omg.org/spec/EDMC-SR/BE/LegalEntities/FormalBusinessOrganizations/isSubUnitOf">
      <skos:definition>The organization is a sub-unit of a Formal Organization and has the role and function of being a formal part of that organization, such as a branch.</skos:definition>
      <rdfs:subPropertyOf rdf:resource="http://www.omg.org/spec/EDMC-SR/FND/Relations/Relations/isPartOf"/>
      <rdfs:domain rdf:resource="http://www.omg.org/spec/EDMC-SR/BE/LegalEntities/FormalBusinessOrganizations/OrganizationalSubUnit"/>
      <rdfs:range rdf:resource="http://www.omg.org/spec/EDMC-SR/BE/LegalEntities/FormalBusinessOrganizations/FormallyConstitutedOrganization"/>
   </owl:ObjectProperty>

   <!--Data Properties-->

<owl:DatatypeProperty rdf:about="http://www.omg.org/spec/EDMC-SR/BE/LegalEntities/FormalBusinessOrganizations/hasUniqueIdentifier">
      <rdfs:range rdf:resource="http://www.omg.org/spec/EDMC-SR/FND/Utilities/BusinessFacingTypes/text"/>
   </owl:DatatypeProperty>

   <!--Annotation Properties-->

<!--Classes-->

<owl:Class rdf:about="http://www.omg.org/spec/EDMC-SR/BE/LegalEntities/FormalBusinessOrganizations/Branch">
      <rdfs:label>Branch</rdfs:label>
      <skos:definition>A part of a business organization or company, identified as a branch.</skos:definition>
      <skos:editorialNote>This is not a separate legal entity in its own right, but a functional part of the entity. [notes not in he issues model Review session 30 March 2011: Branch is vague. Org trades internationally through a branch structure. In retail: The offices people go into to effect their banking. In wholesale: units within the organization that have reporting responsibility to local monetary authorities. The reporting responsibilities are as a result of being a Legal Entity. Bank uses the term "Branch" to reflect that, and is allowed to trade as "NAB Ltd." within those. Other banks would trade as separate legal entities. [The above relates to something other than this definition of "Branch" and belongs elsewhere] Subsidiary - orthogonal to Legal Entity, orthogonal to Reporting responsibility. One node may be a subsidiary AND a Legal Entity and a reporting responsibility / entity. "Branch" just an internal concept. May also be a Legal Entity or not. For those banks that trade in the way NAB does, co is incorporated in Aus but is Registered with monetary authorities elsewhere. Some jurisdictions allow that and some do not (e.g. Switzerland) This is all orthogonal to share ownership "subsidiary". Company is a corpoation but branches may be "Wholly owned subsidiaries" as well. Also the term "Branch" may be the corner office / venue for retail services. For the other kind of Branch: use "Location" to define the other set of terms which use the word "Branch". So separate these meanings. The word to use is "Location". But that need to be teased out. Concept of location as an entity that exists in a location AND the location is addressable. See also semantics of addresses. Clarify address as being an index to a location.</skos:editorialNote>
      <rdfs:subClassOf rdf:resource="http://www.omg.org/spec/EDMC-SR/BE/LegalEntities/FormalBusinessOrganizations/OrganizationalSubUnit"/>
   </owl:Class>

   <owl:Class rdf:about="http://www.omg.org/spec/EDMC-SR/BE/LegalEntities/FormalBusinessOrganizations/Division">
      <rdfs:label>Division</rdfs:label>
      <skos:definition>A part of a company.</skos:definition>
      <skos:editorialNote>[notes not included in issued model] Various kinds of these: Line of Business - e.g. metals, plastic and so on. Department - e.g. Human Resources Division - reporting? Overlaps Line of Business Cost center - in context of accounting only. Internal. Organization sub unit may report on cost or on profit. Overlaps with department. Synonyms - which of these are synonyms. Some terms used interchangeably. If we are to be precise, some of these may have differences but in mot contexts are the same thing. Meanings may have been lost in the mists of time. So they are used interchangeably but which have distinct meanings if we really go down into. Use context to disambiguate these. e.g. Costs / management costs - requires precision on this. There are some org structure concepts not needed here but which are relevant to someone. So they are not really synonyms when we get down to that level. Organizational structure is a topic of its own that can come back to. for now: Definition of internal is a moving feast Depending on context, what's considered internal or not may differ. Decision: 1. things which matter internally - not so interested in these 2. Internally - organizational sub units, are not of interest for now. Decision: model the things we care about, about other organizations. We will not model the things that we care about, about our own business. Come back to the internal stuff as another exercise.</skos:editorialNote>
   </owl:Class>

   <owl:Class rdf:about="http://www.omg.org/spec/EDMC-SR/BE/LegalEntities/FormalBusinessOrganizations/FormalBusinessOrganizationMember">
      <rdfs:label>Formal Business Organization Member</rdfs:label>
      <skos:definition>A member of some Formal Organization.</skos:definition>
      <skos:editorialNote>This party may hold some equity in the Formal Organization and may or may not have some responsibilities or potential liabilitiy in resect of the activities of that organization. Terms setting out the position of the member in these and other matters are defined in the Organization Covering Agreement, to which the Organization Member may be a signatory .</skos:editorialNote>
      <rdfs:subClassOf rdf:resource="http://www.omg.org/spec/EDMC-SR/FND/Parties/Parties/OrganizationMember"/>
   </owl:Class>

   <owl:Class rdf:about="http://www.omg.org/spec/EDMC-SR/BE/LegalEntities/FormalBusinessOrganizations/JointVenture">
      <rdfs:label>Joint Venture</rdfs:label>
      <skos:definition>A formal venture between two or more business entities.</skos:definition>
      <skos:editorialNote>Detailed properties still to be modeled. This will be similar to Partnership in that it will have two or more venture partners (need to determine best label for these), and some formal standing. Also to research: whether JVs are only instituted via mutual share ownership and therefore may only be between limited companies (or may only be a limited company but may have other types of legal person and/or legal entity as venture partners).</skos:editorialNote>
      <rdfs:subClassOf rdf:resource="http://www.omg.org/spec/EDMC-SR/BE/LegalEntities/FormalBusinessOrganizations/FormallyConstitutedOrganization"/>
   </owl:Class>

   <owl:Class rdf:about="http://www.omg.org/spec/EDMC-SR/BE/LegalEntities/FormalBusinessOrganizations/OrganizationCoveringAgreement">
      <rdfs:label>Organization Covering Agreement</rdfs:label>
      <skos:definition>A formal agreement between the principals in a formal organization which covers the relationship between the principals, and between the principals and the entity.</skos:definition>
      <skos:editorialNote>Also covers the aims and purposes of the Entity.</skos:editorialNote>
      <rdfs:subClassOf rdf:resource="http://www.omg.org/spec/EDMC-SR/FND/Agreements/Contracts/WrittenContract"/>
   </owl:Class>

   <owl:Class rdf:about="http://www.omg.org/spec/EDMC-SR/BE/LegalEntities/FormalBusinessOrganizations/OrganizationIdentificationScheme">
      <rdfs:label>Organization Identification Scheme</rdfs:label>
      <skos:definition>A formal scheme defining identification codes for a business entity.</skos:definition>
      <rdfs:subClassOf rdf:resource="http://www.edmcouncil.org/spec/EDMC-SR/FND/Information/Identifiers/IdentificationScheme"/>
   </owl:Class>

   <owl:Class rdf:about="http://www.omg.org/spec/EDMC-SR/BE/LegalEntities/FormalBusinessOrganizations/OrganizationIndustrySectorClassification">
      <rdfs:label>Organization Industry Sector Classification</rdfs:label>
      <skos:definition>The classification of an organization in terms of the industry sector in which it carries out business.</skos:definition>
      <rdfs:subClassOf rdf:resource="http://www.edmcouncil.org/spec/EDMC-SR/FND/Information/Schemes/Classification"/>
   </owl:Class>

   <owl:Class rdf:about="http://www.omg.org/spec/EDMC-SR/BE/LegalEntities/FormalBusinessOrganizations/OrganizationalSubUnit">
      <rdfs:label>Organizational Sub Unit</rdfs:label>
      <skos:definition>An Organization which is part of some larger Formal Organization and only has full recognition within the context of that Formal Organization, it is not a Legal Entity in its own right.</skos:definition>
      <rdfs:subClassOf rdf:resource="http://www.omg.org/spec/EDMC-SR/FND/Organizations/FormalOrganizations/FormalOrganization"/>
   </owl:Class>

   <owl:Class rdf:about="http://www.omg.org/spec/EDMC-SR/BE/LegalEntities/FormalBusinessOrganizations/RegisteredAddress">
      <rdfs:label>Registered Address</rdfs:label>
      <skos:definition>The address at which an entity is registered and at which legal papers may be served.</skos:definition>
      <skos:editorialNote>This usually has to not be a postal address (except in some jurisdictions). So there should be a common superclass.</skos:editorialNote>
      <rdfs:subClassOf rdf:resource="http://www.omg.org/spec/EDMC-SR/FND/Places/Addresses/PostalAddress"/>
   </owl:Class>

   <owl:Class rdf:about="http://www.omg.org/spec/EDMC-SR/BE/LegalEntities/FormalBusinessOrganizations/OrganizationIdentificationCode">
      <rdfs:label>Organization Identification Code</rdfs:label>
      <skos:definition>A textual code which uniquely identifies a formal organization Further Notes Things which may identified by this kind of code Include but are not restricted to Legal Entity. At this most general level, this may be the identifier for a Fund, for a Legal Entity, for a Trust, or for the LEI scope of "Artificial Person plus Trust".</skos:definition>
      <rdfs:subClassOf rdf:resource="http://www.edmcouncil.org/spec/EDMC-SR/FND/Information/Identifiers/Identifier"/>
   </owl:Class>

   <owl:Class rdf:about="http://www.omg.org/spec/EDMC-SR/BE/LegalEntities/FormalBusinessOrganizations/FormallyConstitutedOrganization">
      <rdfs:label>Formally Constituted Organization</rdfs:label>
      <skos:definition>Any organization with some formal contractual agreement among its principals.</skos:definition>
   </owl:Class>

   <!--Individuals-->

</rdf:RDF>