<?xml version="1.0" encoding="UTF-8"?>
<!DOCTYPE rdf:RDF [
	<!ENTITY dct "http://purl.org/dc/terms/">
	<!ENTITY fibo-be-le-cb "https://spec.edmcouncil.org/fibo/BE/LegalEntities/CorporateBodies/">
	<!ENTITY fibo-be-le-fbo "https://spec.edmcouncil.org/fibo/BE/LegalEntities/FormalBusinessOrganizations/">
	<!ENTITY fibo-be-le-lp "https://spec.edmcouncil.org/fibo/BE/LegalEntities/LegalPersons/">
	<!ENTITY fibo-fnd-acc-aeq "https://spec.edmcouncil.org/fibo/FND/Accounting/AccountingEquity/">
	<!ENTITY fibo-fnd-acc-cur "https://spec.edmcouncil.org/fibo/FND/Accounting/CurrencyAmount/">
	<!ENTITY fibo-fnd-law-cor "https://spec.edmcouncil.org/fibo/FND/Law/LegalCore/">
	<!ENTITY fibo-fnd-law-jur "https://spec.edmcouncil.org/fibo/FND/Law/Jurisdiction/">
	<!ENTITY fibo-fnd-org-fm "https://spec.edmcouncil.org/fibo/FND/Organizations/FormalOrganizations/">
	<!ENTITY fibo-fnd-plc-cty "https://spec.edmcouncil.org/fibo/FND/Places/Countries/">
	<!ENTITY fibo-fnd-rel-rel "https://spec.edmcouncil.org/fibo/FND/Relations/Relations/">
	<!ENTITY fibo-fnd-utl-av "https://spec.edmcouncil.org/fibo/FND/Utilities/AnnotationVocabulary/">
	<!ENTITY fibo-fnd-utl-bt "https://spec.edmcouncil.org/fibo/FND/Utilities/BusinessFacingTypes/">
	<!ENTITY owl "http://www.w3.org/2002/07/owl#">
	<!ENTITY rdf "http://www.w3.org/1999/02/22-rdf-syntax-ns#">
	<!ENTITY rdfs "http://www.w3.org/2000/01/rdf-schema#">
	<!ENTITY skos "http://www.w3.org/2004/02/skos/core#">
	<!ENTITY sm "http://www.omg.org/techprocess/ab/SpecificationMetadata/">
	<!ENTITY xsd "http://www.w3.org/2001/XMLSchema#">
]>
<rdf:RDF xml:base="https://spec.edmcouncil.org/fibo/BE/LegalEntities/CorporateBodies/"
	xmlns:dct="http://purl.org/dc/terms/"
	xmlns:fibo-be-le-cb="https://spec.edmcouncil.org/fibo/BE/LegalEntities/CorporateBodies/"
	xmlns:fibo-be-le-fbo="https://spec.edmcouncil.org/fibo/BE/LegalEntities/FormalBusinessOrganizations/"
	xmlns:fibo-be-le-lp="https://spec.edmcouncil.org/fibo/BE/LegalEntities/LegalPersons/"
	xmlns:fibo-fnd-acc-aeq="https://spec.edmcouncil.org/fibo/FND/Accounting/AccountingEquity/"
	xmlns:fibo-fnd-acc-cur="https://spec.edmcouncil.org/fibo/FND/Accounting/CurrencyAmount/"
	xmlns:fibo-fnd-law-cor="https://spec.edmcouncil.org/fibo/FND/Law/LegalCore/"
	xmlns:fibo-fnd-law-jur="https://spec.edmcouncil.org/fibo/FND/Law/Jurisdiction/"
	xmlns:fibo-fnd-org-fm="https://spec.edmcouncil.org/fibo/FND/Organizations/FormalOrganizations/"
	xmlns:fibo-fnd-plc-cty="https://spec.edmcouncil.org/fibo/FND/Places/Countries/"
	xmlns:fibo-fnd-rel-rel="https://spec.edmcouncil.org/fibo/FND/Relations/Relations/"
	xmlns:fibo-fnd-utl-av="https://spec.edmcouncil.org/fibo/FND/Utilities/AnnotationVocabulary/"
	xmlns:fibo-fnd-utl-bt="https://spec.edmcouncil.org/fibo/FND/Utilities/BusinessFacingTypes/"
	xmlns:owl="http://www.w3.org/2002/07/owl#"
	xmlns:rdf="http://www.w3.org/1999/02/22-rdf-syntax-ns#"
	xmlns:rdfs="http://www.w3.org/2000/01/rdf-schema#"
	xmlns:skos="http://www.w3.org/2004/02/skos/core#"
	xmlns:sm="http://www.omg.org/techprocess/ab/SpecificationMetadata/"
	xmlns:xsd="http://www.w3.org/2001/XMLSchema#">
	
	<owl:Ontology rdf:about="https://spec.edmcouncil.org/fibo/BE/LegalEntities/CorporateBodies/">
		<rdfs:label>Corporate Bodies Ontology</rdfs:label>
		<dct:license rdf:datatype="&xsd;anyURI">http://opensource.org/licenses/MIT</dct:license>
		<sm:contentLanguage rdf:datatype="&xsd;anyURI">http://www.omg.org/spec/ODM/</sm:contentLanguage>
		<sm:contentLanguage rdf:datatype="&xsd;anyURI">http://www.w3.org/standards/techs/owl#w3c_all</sm:contentLanguage>
		<sm:copyright>Copyright (c) 2013-2016 EDM Council, Inc.
Copyright (c) 2013-2016 Object Management Group, Inc.</sm:copyright>
		<sm:dependsOn rdf:datatype="&xsd;anyURI">https://spec.edmcouncil.org/fibo/BE/LegalEntities/FormalBusinessOrganizations/</sm:dependsOn>
		<sm:dependsOn rdf:datatype="&xsd;anyURI">https://spec.edmcouncil.org/fibo/BE/LegalEntities/LegalPersons/</sm:dependsOn>
		<sm:dependsOn rdf:datatype="&xsd;anyURI">https://spec.edmcouncil.org/fibo/FND/</sm:dependsOn>
		<sm:fileAbbreviation>fibo-be-le-cb</sm:fileAbbreviation>
		<dct:abstract>This ontology defines the basic mechanisms that establish legal personhood for judicial or artificial persons, specifically those that are corporate bodies, including bodies incorporated by equity, by guarantee, and by agreement.</dct:abstract>
		<sm:filename>CorporateBodies.rdf</sm:filename>
		<rdfs:seeAlso rdf:datatype="&xsd;anyURI">https://spec.edmcouncil.org/fibo/AboutTheEDMC-FIBOFamily/</rdfs:seeAlso>
		<rdfs:seeAlso rdf:datatype="&xsd;anyURI">https://spec.edmcouncil.org/fibo/BE/AboutBE/</rdfs:seeAlso>
		<rdfs:seeAlso rdf:datatype="&xsd;anyURI">https://spec.edmcouncil.org/fibo/BE/LegalEntities/AboutLegalEntities/</rdfs:seeAlso>
		<owl:imports rdf:resource="https://spec.edmcouncil.org/fibo/BE/LegalEntities/FormalBusinessOrganizations/"/>
		<owl:imports rdf:resource="https://spec.edmcouncil.org/fibo/BE/LegalEntities/LegalPersons/"/>
		<owl:imports rdf:resource="https://spec.edmcouncil.org/fibo/FND/Accounting/AccountingEquity/"/>
		<owl:imports rdf:resource="https://spec.edmcouncil.org/fibo/FND/Accounting/CurrencyAmount/"/>
		<owl:imports rdf:resource="https://spec.edmcouncil.org/fibo/FND/Law/Jurisdiction/"/>
		<owl:imports rdf:resource="https://spec.edmcouncil.org/fibo/FND/Law/LegalCore/"/>
		<owl:imports rdf:resource="https://spec.edmcouncil.org/fibo/FND/Organizations/FormalOrganizations/"/>
		<owl:imports rdf:resource="https://spec.edmcouncil.org/fibo/FND/Places/Countries/"/>
		<owl:imports rdf:resource="https://spec.edmcouncil.org/fibo/FND/Relations/Relations/"/>
		<owl:imports rdf:resource="https://spec.edmcouncil.org/fibo/FND/Utilities/AnnotationVocabulary/"/>
		<owl:imports rdf:resource="https://spec.edmcouncil.org/fibo/FND/Utilities/BusinessFacingTypes/"/>
		<owl:versionIRI rdf:resource="https://spec.edmcouncil.org/fibo/BE/20160201/LegalEntities/CorporateBodies/"/>
		<skos:changeNote>The https://spec.edmcouncil.org/fibo/BE/20131101/LegalEntities/CorporateBodies.rdf version of this ontology was modified per the issue resolutions identified in the FIBO BE 1.0 FTF report.</skos:changeNote>
		<fibo-fnd-utl-av:hasMaturityLevel rdf:resource="&fibo-fnd-utl-av;Release"/>
	</owl:Ontology>
	
	<owl:Class rdf:about="&fibo-be-le-cb;BenefitCorporation">
		<rdfs:subClassOf rdf:resource="&fibo-be-le-cb;NotForProfitCorporation"/>
		<rdfs:label>benefit corporation</rdfs:label>
		<rdfs:seeAlso rdf:datatype="&xsd;anyURI">http://www.business.ca.gov/Portals/0/Home/Docs/AB%202641%20SOS.pdf</rdfs:seeAlso>
		<skos:definition>a not for profit corporation set up under specific state legislation to provide some stated societal benefit, and with some corresponding relaxation of the obligation to maximize shareholder return</skos:definition>
		<fibo-fnd-utl-av:adaptedFrom rdf:datatype="&xsd;anyURI">www.bcorporation.net</fibo-fnd-utl-av:adaptedFrom>
		<fibo-fnd-utl-av:explanatoryNote>This is a US-specific type of non-profit corporation defined in recent legislation in a number of states. In California, for example, benefit corporations may be defined as public benefit or mutual benefit corporations, depending on their purpose.</fibo-fnd-utl-av:explanatoryNote>
	</owl:Class>
	
	<owl:Class rdf:about="&fibo-be-le-cb;BodyIncorporatedThroughAgreement">
		<rdfs:subClassOf rdf:resource="&fibo-be-le-cb;Corporation"/>
		<rdfs:label>body incorporated through agreement</rdfs:label>
		<skos:definition>A body with legal personhood, incorporated through some agreement among the principals, and without equity or guarantee instruments which would isolate the principals from liability.</skos:definition>
		<skos:editorialNote>An LLP (in the UK) is an example of this, and is also a partnership. There, the LLP Document is the legal document which effectively constitutes the Partnership.</skos:editorialNote>
	</owl:Class>
	
	<owl:Class rdf:about="&fibo-be-le-cb;BodyIncorporatedWithGuarantee">
		<rdfs:subClassOf rdf:resource="&fibo-be-le-cb;Corporation"/>
		<rdfs:subClassOf>
			<owl:Restriction>
				<owl:onProperty rdf:resource="&fibo-fnd-rel-rel;isGovernedBy"/>
				<owl:onClass rdf:resource="&fibo-be-le-cb;BodyLimitedByGuaranteePrincipalsAgreement"/>
				<owl:minQualifiedCardinality rdf:datatype="&xsd;nonNegativeInteger">0</owl:minQualifiedCardinality>
			</owl:Restriction>
		</rdfs:subClassOf>
		<rdfs:label>body incorporated with guarantee</rdfs:label>
		<owl:disjointWith rdf:resource="&fibo-be-le-cb;BodyIncorporatedThroughAgreement"/>
		<skos:definition>Incorporated entity without share capital, and in which the liability of its members is limited to the amount each one of them undertakes to contribute at the time the firm is wound up.</skos:definition>
		<skos:editorialNote>The profit motive is not the prime objective of the organization.</skos:editorialNote>
	</owl:Class>
	
	<owl:Class rdf:about="&fibo-be-le-cb;BodyLimitedByGuaranteePrincipalsAgreement">
		<rdfs:subClassOf rdf:resource="&fibo-be-le-fbo;OrganizationCoveringAgreement"/>
		<rdfs:label>body limited by guarantee principals agreement</rdfs:label>
		<skos:definition>The formal agreement between the principals of a body limited by guarantee.</skos:definition>
	</owl:Class>
	
	<owl:Class rdf:about="&fibo-be-le-cb;CommonInterestDevelopmentCorporation">
		<rdfs:subClassOf rdf:resource="&fibo-be-le-cb;NotForProfitCorporation"/>
		<rdfs:label>common interest development corporation</rdfs:label>
		<skos:definition>a not for profit corporation set up under specific state legislation as a business entity for homeowners&apos; associations</skos:definition>
		<skos:example rdf:datatype="&xsd;anyURI">http://www.dre.ca.gov/files/pdf/re39.pdf</skos:example>
		<fibo-fnd-utl-av:adaptedFrom rdf:datatype="&xsd;anyURI">http://www.nolo.com/dictionary/common-interest-development-term.html</fibo-fnd-utl-av:adaptedFrom>
		<fibo-fnd-utl-av:explanatoryNote>A common interest development is typically a type of housing, composed of individually owned units, such as condominiums, townhouses, or single-family homes, that share ownership of common areas, such as swimming pools, landscaping, and parking. Common interest developments (also known as community interest developments or CIDs) are managed by homeowners&apos; associations.</fibo-fnd-utl-av:explanatoryNote>
	</owl:Class>
	
	<owl:Class rdf:about="&fibo-be-le-cb;CompanyIncorporatedByGuarantee">
		<rdfs:subClassOf rdf:resource="&fibo-be-le-cb;BodyIncorporatedWithGuarantee"/>
		<rdfs:label>company incorporated by guarantee</rdfs:label>
		<fibo-fnd-utl-av:definitionOrigin>www.investorwords.com</fibo-fnd-utl-av:definitionOrigin>
	</owl:Class>
	
	<owl:Class rdf:about="&fibo-be-le-cb;Corporation">
		<rdfs:subClassOf rdf:resource="&fibo-be-le-fbo;FormallyConstitutedOrganization"/>
		<rdfs:subClassOf rdf:resource="&fibo-be-le-lp;JuridicalPerson"/>
		<rdfs:subClassOf>
			<owl:Restriction>
				<owl:onProperty rdf:resource="&fibo-fnd-org-fm;isDomiciledIn"/>
				<owl:onClass rdf:resource="&fibo-fnd-plc-cty;Country"/>
				<owl:minQualifiedCardinality rdf:datatype="&xsd;nonNegativeInteger">1</owl:minQualifiedCardinality>
			</owl:Restriction>
		</rdfs:subClassOf>
		<rdfs:subClassOf>
			<owl:Restriction>
				<owl:onProperty rdf:resource="&fibo-fnd-rel-rel;hasLegalName"/>
				<owl:minQualifiedCardinality rdf:datatype="&xsd;nonNegativeInteger">1</owl:minQualifiedCardinality>
				<owl:onDataRange rdf:resource="&fibo-fnd-utl-bt;text"/>
			</owl:Restriction>
		</rdfs:subClassOf>
		<rdfs:subClassOf>
			<owl:Restriction>
				<owl:onProperty rdf:resource="&fibo-be-le-cb;isConstitutedBy"/>
				<owl:onClass rdf:resource="&fibo-be-le-cb;InstrumentOfIncorporation"/>
				<owl:qualifiedCardinality rdf:datatype="&xsd;nonNegativeInteger">1</owl:qualifiedCardinality>
			</owl:Restriction>
		</rdfs:subClassOf>
		<rdfs:subClassOf>
			<owl:Restriction>
				<owl:onProperty rdf:resource="&fibo-be-le-cb;isIncorporatedIn"/>
				<owl:onClass rdf:resource="&fibo-fnd-law-jur;Jurisdiction"/>
				<owl:qualifiedCardinality rdf:datatype="&xsd;nonNegativeInteger">1</owl:qualifiedCardinality>
			</owl:Restriction>
		</rdfs:subClassOf>
		<rdfs:label xml:lang="en">corporation</rdfs:label>
		<skos:definition>a formal organization treated as an entity - an artificial person or legal entity distinct from its owners - created by or under the authority of the laws of a state or nation</skos:definition>
		<fibo-fnd-utl-av:adaptedFrom>Barron&apos;s Dictionary of Banking Terms, Sixth Edition, 2012, definition of corporation</fibo-fnd-utl-av:adaptedFrom>
		<fibo-fnd-utl-av:adaptedFrom rdf:datatype="&xsd;anyURI">http://thelawdictionary.org/corporation/</fibo-fnd-utl-av:adaptedFrom>
		<fibo-fnd-utl-av:explanatoryNote>A corporation has three distinguishing characteristics: (1) separation of ownership from management and general liability, i.e., its liability to creditors is limited to its resources, unlike some partnerships and sole proprietorships, (2) the ability to negotiate contracts and own property, and (3) transferable ownership, irrespective of changes in membership or the lifetimes of its stockholders.</fibo-fnd-utl-av:explanatoryNote>
		<fibo-fnd-utl-av:explanatoryNote>A corporation is managed by or under the direction of a board of directors, which generally determines corporate policy. Officers manage the day-to-day affairs of the corporation.</fibo-fnd-utl-av:explanatoryNote>
		<fibo-fnd-utl-av:synonym>body corporate</fibo-fnd-utl-av:synonym>
	</owl:Class>
	
	<owl:Class rdf:about="&fibo-be-le-cb;ForProfitCorporation">
		<rdfs:subClassOf rdf:resource="&fibo-be-le-cb;Corporation"/>
		<rdfs:subClassOf>
			<owl:Restriction>
				<owl:onProperty rdf:resource="&fibo-be-le-lp;hasObjective"/>
				<owl:someValuesFrom rdf:resource="&fibo-be-le-lp;ProfitObjective"/>
			</owl:Restriction>
		</rdfs:subClassOf>
		<rdfs:label>for profit corporation</rdfs:label>
		<owl:disjointWith rdf:resource="&fibo-be-le-cb;NotForProfitCorporation"/>
		<skos:definition>a corporation whose objective is to make money, in other words, to ensure realization of a financial benefit such that the amount of revenue gained from a business activity exceeds the expenses, costs and taxes needed to sustain that activity</skos:definition>
		<fibo-fnd-utl-av:adaptedFrom rdf:datatype="&xsd;anyURI">http://www.investopedia.com/terms/p/profit.asp</fibo-fnd-utl-av:adaptedFrom>
	</owl:Class>
	
	<owl:Class rdf:about="&fibo-be-le-cb;IncorporationGuarantee">
		<rdfs:subClassOf rdf:resource="&fibo-fnd-law-cor;Constitution"/>
		<rdfs:subClassOf>
			<owl:Restriction>
				<owl:onProperty rdf:resource="&fibo-fnd-rel-rel;isProvidedBy"/>
				<owl:cardinality rdf:datatype="&xsd;nonNegativeInteger">1</owl:cardinality>
			</owl:Restriction>
		</rdfs:subClassOf>
		<rdfs:subClassOf>
			<owl:Restriction>
				<owl:onProperty rdf:resource="&fibo-fnd-acc-cur;hasNotionalAmount"/>
				<owl:onClass rdf:resource="&fibo-fnd-acc-cur;MonetaryAmount"/>
				<owl:qualifiedCardinality rdf:datatype="&xsd;nonNegativeInteger">1</owl:qualifiedCardinality>
			</owl:Restriction>
		</rdfs:subClassOf>
		<rdfs:label>incorporation guarantee</rdfs:label>
		<skos:definition>A guarantee which is part of the means by which some incorporated entity is incorporated by guarantee.</skos:definition>
	</owl:Class>
	
	<owl:Class rdf:about="&fibo-be-le-cb;InstrumentOfIncorporation">
		<rdfs:subClassOf rdf:resource="&fibo-fnd-law-cor;Constitution"/>
		<rdfs:subClassOf>
			<owl:Restriction>
				<owl:onProperty rdf:resource="&fibo-fnd-rel-rel;isGovernedBy"/>
				<owl:onClass rdf:resource="&fibo-fnd-law-jur;Jurisdiction"/>
				<owl:qualifiedCardinality rdf:datatype="&xsd;nonNegativeInteger">1</owl:qualifiedCardinality>
			</owl:Restriction>
		</rdfs:subClassOf>
		<rdfs:label>instrument of incorporation</rdfs:label>
		<skos:definition>Some legal instrument by which some legal entity which is not a natural person is made to exist.</skos:definition>
		<skos:editorialNote>This may be the issuance of shares, the existence of some agreement, guaranties and so on.</skos:editorialNote>
	</owl:Class>
	
	<owl:Class rdf:about="&fibo-be-le-cb;NotForProfitCorporation">
		<rdfs:subClassOf rdf:resource="&fibo-be-le-cb;Corporation"/>
		<rdfs:subClassOf rdf:resource="&fibo-be-le-fbo;NotForProfitOrganization"/>
		<rdfs:label>not for profit corporation</rdfs:label>
		<skos:definition>a corporation approved by its jurisdictional oversight and taxing authorities as operating for educational, charitable, social, religious, civic or humanitarian purposes</skos:definition>
		<fibo-fnd-utl-av:adaptedFrom rdf:datatype="&xsd;anyURI">http://legal-dictionary.thefreedictionary.com/nonprofit+corporation</fibo-fnd-utl-av:adaptedFrom>
		<fibo-fnd-utl-av:explanatoryNote>A not for profit corporation is formed by incorporators, and has a board of directors and officers, but no shareholders. These incorporators, directors and officers may not receive a distribution of (any money from) profits, but officers and management may be paid reasonable salaries for services to the corporation.</fibo-fnd-utl-av:explanatoryNote>
		<fibo-fnd-utl-av:synonym>non-profit corporation</fibo-fnd-utl-av:synonym>
	</owl:Class>
	
	<owl:Class rdf:about="&fibo-be-le-cb;StockCorporation">
		<rdfs:subClassOf rdf:resource="&fibo-be-le-cb;Corporation"/>
		<rdfs:subClassOf>
			<owl:Restriction>
				<owl:onProperty rdf:resource="&fibo-be-le-cb;issuesEquity"/>
				<owl:someValuesFrom rdf:resource="&fibo-fnd-acc-aeq;IssuedEquity"/>
			</owl:Restriction>
		</rdfs:subClassOf>
		<rdfs:label xml:lang="en">stock corporation</rdfs:label>
		<owl:disjointWith rdf:resource="&fibo-be-le-cb;BodyIncorporatedThroughAgreement"/>
		<owl:disjointWith rdf:resource="&fibo-be-le-cb;BodyIncorporatedWithGuarantee"/>
		<skos:definition>a corporation that has shareholders (stockholders), each of whom receives a portion of the ownership of the corporation through shares of stock</skos:definition>
		<fibo-fnd-utl-av:adaptedFrom rdf:datatype="&xsd;anyURI">http://biztaxlaw.about.com/od/glossarys/g/stockcorp.htm</fibo-fnd-utl-av:adaptedFrom>
		<fibo-fnd-utl-av:adaptedFrom rdf:datatype="&xsd;anyURI">http://www.oecd.org/daf/ca/CorporateGovernanceFactbook.pdf</fibo-fnd-utl-av:adaptedFrom>
		<fibo-fnd-utl-av:explanatoryNote>The shares in a stock corporation may receive a return on their investment in the form of dividends. Shares are used for voting on matters of corporate policy or to elect directors, at the corporation&apos;s annual meeting and at other meetings of the corporation.</fibo-fnd-utl-av:explanatoryNote>
	</owl:Class>
	
	<owl:ObjectProperty rdf:about="&fibo-be-le-cb;isConstitutedBy">
		<rdfs:label>is constituted by</rdfs:label>
		<rdfs:domain rdf:resource="&fibo-be-le-cb;Corporation"/>
		<rdfs:range rdf:resource="&fibo-fnd-law-cor;Constitution"/>
		<skos:definition>the instrument by which an entity is incorporated</skos:definition>
	</owl:ObjectProperty>
	
	<owl:ObjectProperty rdf:about="&fibo-be-le-cb;isIncorporatedIn">
		<rdfs:subPropertyOf rdf:resource="&fibo-be-le-lp;isOrganizedIn"/>
		<rdfs:label>is incorporated in</rdfs:label>
		<rdfs:domain rdf:resource="&fibo-be-le-cb;Corporation"/>
		<rdfs:range rdf:resource="&fibo-fnd-law-jur;Jurisdiction"/>
		<skos:definition>the legal jurisdiction under which the legal entity is incorporated</skos:definition>
		<skos:editorialNote>It is the laws of this jurisdiction that cause and allow the legal entity to exist and to incur debt and be sued at law as a legal entity.</skos:editorialNote>
	</owl:ObjectProperty>
	
	<owl:ObjectProperty rdf:about="&fibo-be-le-cb;issuesEquity">
		<rdfs:label>issues equity</rdfs:label>
		<rdfs:domain rdf:resource="&fibo-be-le-cb;StockCorporation"/>
		<rdfs:range rdf:resource="&fibo-fnd-acc-aeq;IssuedEquity"/>
		<skos:definition>relates a stock corporation to the equity (in the form of shares) it issues through incorporation and subsequent corporate actions</skos:definition>
	</owl:ObjectProperty>

</rdf:RDF>
