<?xml version="1.0" encoding="UTF-8"?>
<!DOCTYPE rdf:RDF [
	<!ENTITY fibo-be-fct-fct "https://spec.edmcouncil.org/fibo/BE/FunctionalEntities/FunctionalEntities/">
	<!ENTITY fibo-be-fctx-brn "https://spec.edmcouncil.org/fibo/BE/FunctionalEntitiesExt/Branding/">
	<!ENTITY fibo-fnd-inf-inf "https://spec.edmcouncil.org/fibo/FND/InformationExt/InfoCore/">
	<!ENTITY fibo-fnd-utl-av "https://spec.edmcouncil.org/fibo/FND/Utilities/AnnotationVocabulary/">
	<!ENTITY owl "http://www.w3.org/2002/07/owl#">
	<!ENTITY rdf "http://www.w3.org/1999/02/22-rdf-syntax-ns#">
	<!ENTITY rdfs "http://www.w3.org/2000/01/rdf-schema#">
	<!ENTITY skos "http://www.w3.org/2004/02/skos/core#">
	<!ENTITY xsd "http://www.w3.org/2001/XMLSchema#">
]>
<rdf:RDF xml:base="https://spec.edmcouncil.org/fibo/BE/FunctionalEntitiesExt/Branding/"
	xmlns:fibo-be-fct-fct="https://spec.edmcouncil.org/fibo/BE/FunctionalEntities/FunctionalEntities/"
	xmlns:fibo-be-fctx-brn="https://spec.edmcouncil.org/fibo/BE/FunctionalEntitiesExt/Branding/"
	xmlns:fibo-fnd-inf-inf="https://spec.edmcouncil.org/fibo/FND/InformationExt/InfoCore/"
	xmlns:fibo-fnd-utl-av="https://spec.edmcouncil.org/fibo/FND/Utilities/AnnotationVocabulary/"
	xmlns:owl="http://www.w3.org/2002/07/owl#"
	xmlns:rdf="http://www.w3.org/1999/02/22-rdf-syntax-ns#"
	xmlns:rdfs="http://www.w3.org/2000/01/rdf-schema#"
	xmlns:skos="http://www.w3.org/2004/02/skos/core#"
	xmlns:xsd="http://www.w3.org/2001/XMLSchema#">
	
	<owl:Ontology rdf:about="https://spec.edmcouncil.org/fibo/BE/FunctionalEntitiesExt/Branding/">
		<rdfs:label xml:lang="en">Branding</rdfs:label>
		<owl:imports rdf:resource="http://www.w3.org/2004/02/skos/core"/>
		<owl:imports rdf:resource="https://spec.edmcouncil.org/fibo/BE/FunctionalEntities/FunctionalEntities/"/>
		<owl:imports rdf:resource="https://spec.edmcouncil.org/fibo/FND/InformationExt/InfoCore/"/>
		<owl:imports rdf:resource="https://spec.edmcouncil.org/fibo/FND/Utilities/AnnotationVocabulary/"/>
		<owl:versionIRI rdf:resource="https://spec.edmcouncil.org/fibo/BE/FunctionalEntitiesExt/Branding/"/>
		<fibo-fnd-utl-av:hasMaturityLevel rdf:resource="&fibo-fnd-utl-av;Informative"/>
	</owl:Ontology>
	
	<owl:Class rdf:about="&fibo-be-fct-fct;Business">
		<owl:equivalentClass rdf:resource="&fibo-be-fctx-brn;Business"/>
	</owl:Class>
	
	<owl:Class rdf:about="&fibo-be-fctx-brn;BrandName">
		<rdfs:subClassOf rdf:resource="&fibo-fnd-inf-inf;Name"/>
		<rdfs:label xml:lang="en">brand name</rdfs:label>
		<skos:definition xml:lang="en">A name with or without some strong image (usually legally defined), which identifies an organization or some part of product or service thereof.</skos:definition>
	</owl:Class>
	
	<owl:Class rdf:about="&fibo-be-fctx-brn;Business">
		<rdfs:subClassOf>
			<owl:Restriction>
				<owl:onProperty rdf:resource="&fibo-be-fctx-brn;hasCommercialIdentity"/>
				<owl:someValuesFrom rdf:resource="&fibo-be-fctx-brn;BrandName"/>
			</owl:Restriction>
		</rdfs:subClassOf>
		<rdfs:label xml:lang="en">business</rdfs:label>
		<skos:definition xml:lang="en">Some entity set up for the purposes of carrying out some commercial activities for profit.</skos:definition>
	</owl:Class>
	
	<owl:ObjectProperty rdf:about="&fibo-be-fctx-brn;hasCommercialIdentity">
		<rdfs:subPropertyOf rdf:resource="&fibo-fnd-inf-inf;hasName"/>
		<rdfs:label xml:lang="en">has commercial identity</rdfs:label>
		<rdfs:domain rdf:resource="&fibo-be-fctx-brn;Business"/>
		<rdfs:range rdf:resource="&fibo-be-fctx-brn;BrandName"/>
		<skos:definition xml:lang="en">A name or identity by which a business organization is known for marketing and communication purposes. This may or may not be the same as the name of the organization.</skos:definition>
	</owl:ObjectProperty>

</rdf:RDF>