<?xml version="1.0" encoding="UTF-8"?>
<!DOCTYPE rdf:RDF [
	<!ENTITY fibo-be-fct-fct "https://spec.edmcouncil.org/fibo/BE/FunctionalEntities/FunctionalEntities/">
	<!ENTITY fibo-be-fctx-spv "https://spec.edmcouncil.org/fibo/BE/FunctionalEntitiesExt/SPVs/">
	<!ENTITY fibo-be-le-fbo "https://spec.edmcouncil.org/fibo/BE/LegalEntities/FormalBusinessOrganizations/">
	<!ENTITY fibo-be-le-lp "https://spec.edmcouncil.org/fibo/BE/LegalEntities/LegalPersons/">
	<!ENTITY fibo-fnd-arrxx-ins "https://spec.edmcouncil.org/fibo/FND/ArrangementsExt/ToolsAndInstruments/">
	<!ENTITY fibo-fnd-dt-fd "https://spec.edmcouncil.org/fibo/FND/DatesAndTimes/FinancialDates/">
	<!ENTITY fibo-fnd-utl-av "https://spec.edmcouncil.org/fibo/FND/Utilities/AnnotationVocabulary/">
	<!ENTITY owl "http://www.w3.org/2002/07/owl#">
	<!ENTITY rdf "http://www.w3.org/1999/02/22-rdf-syntax-ns#">
	<!ENTITY rdfs "http://www.w3.org/2000/01/rdf-schema#">
	<!ENTITY skos "http://www.w3.org/2004/02/skos/core#">
	<!ENTITY xsd "http://www.w3.org/2001/XMLSchema#">
]>
<rdf:RDF xml:base="https://spec.edmcouncil.org/fibo/BE/FunctionalEntitiesExt/SPVs/"
	xmlns:fibo-be-fct-fct="https://spec.edmcouncil.org/fibo/BE/FunctionalEntities/FunctionalEntities/"
	xmlns:fibo-be-fctx-spv="https://spec.edmcouncil.org/fibo/BE/FunctionalEntitiesExt/SPVs/"
	xmlns:fibo-be-le-fbo="https://spec.edmcouncil.org/fibo/BE/LegalEntities/FormalBusinessOrganizations/"
	xmlns:fibo-be-le-lp="https://spec.edmcouncil.org/fibo/BE/LegalEntities/LegalPersons/"
	xmlns:fibo-fnd-arrxx-ins="https://spec.edmcouncil.org/fibo/FND/ArrangementsExt/ToolsAndInstruments/"
	xmlns:fibo-fnd-dt-fd="https://spec.edmcouncil.org/fibo/FND/DatesAndTimes/FinancialDates/"
	xmlns:fibo-fnd-utl-av="https://spec.edmcouncil.org/fibo/FND/Utilities/AnnotationVocabulary/"
	xmlns:owl="http://www.w3.org/2002/07/owl#"
	xmlns:rdf="http://www.w3.org/1999/02/22-rdf-syntax-ns#"
	xmlns:rdfs="http://www.w3.org/2000/01/rdf-schema#"
	xmlns:skos="http://www.w3.org/2004/02/skos/core#"
	xmlns:xsd="http://www.w3.org/2001/XMLSchema#">
	
	<owl:Ontology rdf:about="https://spec.edmcouncil.org/fibo/BE/FunctionalEntitiesExt/SPVs/">
		<rdfs:label xml:lang="en">SPVs</rdfs:label>
		<owl:imports rdf:resource="http://www.w3.org/2004/02/skos/core"/>
		<owl:imports rdf:resource="https://spec.edmcouncil.org/fibo/BE/FunctionalEntities/FunctionalEntities/"/>
		<owl:imports rdf:resource="https://spec.edmcouncil.org/fibo/BE/LegalEntities/FormalBusinessOrganizations/"/>
		<owl:imports rdf:resource="https://spec.edmcouncil.org/fibo/BE/LegalEntities/LegalPersons/"/>
		<owl:imports rdf:resource="https://spec.edmcouncil.org/fibo/FND/ArrangementsExt/ToolsAndInstruments/"/>
		<owl:imports rdf:resource="https://spec.edmcouncil.org/fibo/FND/DatesAndTimes/FinancialDates/"/>
		<owl:imports rdf:resource="https://spec.edmcouncil.org/fibo/FND/Utilities/AnnotationVocabulary/"/>
		<owl:imports rdf:resource="https://spec.edmcouncil.org/fibo/SEC/Securities/Pools/"/>
		<owl:versionIRI rdf:resource="https://spec.edmcouncil.org/fibo/BE/FunctionalEntitiesExt/SPVs/"/>
		<fibo-fnd-utl-av:hasMaturityLevel rdf:resource="&fibo-fnd-utl-av;Informative"/>
	</owl:Ontology>
	
	<owl:Class rdf:about="&fibo-be-fctx-spv;SPVPurpose">
		<rdfs:subClassOf rdf:resource="&fibo-fnd-arrxx-ins;Purpose"/>
		<rdfs:label xml:lang="en">s p v purpose</rdfs:label>
		<skos:definition xml:lang="en">The reason for the creation of a Special Purpose Vehicle.</skos:definition>
		<skos:editorialNote xml:lang="en">This is used to identify different kinds of SPV which may have different detailed facts about them; however in general all SPVs are much the same.</skos:editorialNote>
	</owl:Class>
	
	<owl:Class rdf:about="&fibo-be-fctx-spv;SpecialPurposeVehicle">
		<rdfs:subClassOf rdf:resource="&fibo-be-fct-fct;FunctionalBusinessEntity"/>
		<rdfs:subClassOf>
			<owl:Restriction>
				<owl:onProperty rdf:resource="&fibo-be-fctx-spv;constitutedAs"/>
				<owl:someValuesFrom rdf:resource="&fibo-be-le-fbo;FormallyConstitutedOrganization"/>
			</owl:Restriction>
		</rdfs:subClassOf>
		<rdfs:subClassOf>
			<owl:Restriction>
				<owl:onProperty rdf:resource="&fibo-be-fctx-spv;isSetUpFor"/>
				<owl:someValuesFrom rdf:resource="&fibo-be-fctx-spv;SPVPurpose"/>
			</owl:Restriction>
		</rdfs:subClassOf>
		<rdfs:subClassOf>
			<owl:Restriction>
				<owl:onProperty rdf:resource="&fibo-be-fctx-spv;sPVHoldsPool"/>
				<owl:someValuesFrom rdf:resource="https://spec.edmcouncil.org/fibo/SEC/Securities/Pools/Pool"/>
			</owl:Restriction>
		</rdfs:subClassOf>
		<rdfs:subClassOf>
			<owl:Restriction>
				<owl:onProperty rdf:resource="&fibo-be-fctx-spv;sponsoredBy"/>
				<owl:someValuesFrom rdf:resource="&fibo-be-le-lp;LegalPerson"/>
			</owl:Restriction>
		</rdfs:subClassOf>
		<rdfs:label xml:lang="en">special purpose vehicle</rdfs:label>
		<skos:definition xml:lang="en">A Special Purpose Vehicle (SPV) set up specifically to issue a security or securities. It is set up by a company or a group of companies for some purpose such as to create instruments that are off the company&apos;s balance sheet or to issue Participation Notes for investors in another jurisdiction. The SPV is formed for a specific reason and exists for a specific period of time and is then disbanded. Further notes: Special Purpose Vehicles are also referred to as bankruptcy remote entities, as they isolate financial risk. For Participation Notes: slightly different purpose but the same kind of vehicle. The only investment made by the SPV is that they buy in the stock. These are the same kind of entity in all of the contexts in which they exist.</skos:definition>
	</owl:Class>
	
	<owl:ObjectProperty rdf:about="&fibo-be-fctx-spv;constitutedAs">
		<rdfs:label xml:lang="en">constituted as</rdfs:label>
		<rdfs:domain rdf:resource="&fibo-be-fctx-spv;SpecialPurposeVehicle"/>
		<rdfs:range rdf:resource="&fibo-be-le-fbo;FormallyConstitutedOrganization"/>
		<skos:definition xml:lang="en">The Special Purpose Vehicle is constituted as some kind of Formal Organization.</skos:definition>
		<fibo-fnd-utl-av:explanatoryNote xml:lang="en">This may be a company incorporated by shares, a limited liability company or some other form of legal entity, including legal person and non incorporated formal organization. These are usually limited in their articles as to what they can do. It is as this entity that the SPV is able to be party to contracts and incur debts. Note that it cannot be an individual human being.</fibo-fnd-utl-av:explanatoryNote>
	</owl:ObjectProperty>
	
	<owl:ObjectProperty rdf:about="&fibo-be-fctx-spv;intendedLiquidationDate">
		<rdfs:label xml:lang="en">intended liquidation date</rdfs:label>
		<rdfs:domain rdf:resource="&fibo-be-fctx-spv;SpecialPurposeVehicle"/>
		<rdfs:range rdf:resource="&fibo-fnd-dt-fd;Date"/>
		<skos:definition xml:lang="en">The date on which the SPV is scheduled to be disbanded and wound up.</skos:definition>
	</owl:ObjectProperty>
	
	<owl:ObjectProperty rdf:about="&fibo-be-fctx-spv;isSetUpFor">
		<rdfs:label xml:lang="en">is set up for</rdfs:label>
		<rdfs:domain rdf:resource="&fibo-be-fctx-spv;SpecialPurposeVehicle"/>
		<rdfs:range rdf:resource="&fibo-be-fctx-spv;SPVPurpose"/>
	</owl:ObjectProperty>
	
	<owl:ObjectProperty rdf:about="&fibo-be-fctx-spv;sPVHoldsPool">
		<rdfs:label xml:lang="en">s p v holds pool</rdfs:label>
		<rdfs:domain rdf:resource="&fibo-be-fctx-spv;SpecialPurposeVehicle"/>
		<rdfs:range rdf:resource="https://spec.edmcouncil.org/fibo/SEC/Securities/Pools/Pool"/>
		<skos:definition xml:lang="en">A Special Purpose Vehicle always holds some kind of pool. This may be a debt pool, an asset pool (fund) or some pool of securities from which it issues Participation Notes.</skos:definition>
	</owl:ObjectProperty>
	
	<owl:ObjectProperty rdf:about="&fibo-be-fctx-spv;sponsoredBy">
		<rdfs:label xml:lang="en">sponsored by</rdfs:label>
		<rdfs:domain rdf:resource="&fibo-be-fctx-spv;SpecialPurposeVehicle"/>
		<rdfs:range rdf:resource="&fibo-be-le-lp;LegalPerson"/>
		<skos:definition xml:lang="en">The entity which is the creator and servicer of the SPV. Notes: To protect investors from possible bankruptcy of the corporation, there are three legal safeguards: - Transfer of assets from the corporation is a non-recourse, true sale. - Investors receive a perfected interest in the assets&apos; cash flows. - A non-consolidation legal opinion is obtained certifying that assets of the trust or special purpose vehicle cannot be consolidated with the corporation&apos;s assets in the event of bankruptcy.</skos:definition>
	</owl:ObjectProperty>

</rdf:RDF>