<?xml version="1.0" encoding="UTF-8"?>
<!DOCTYPE rdf:RDF [
	<!ENTITY dct "http://purl.org/dc/terms/">
	<!ENTITY fibo-be-fct-fct "https://spec.edmcouncil.org/fibo/ontology/BE/FunctionalEntities/FunctionalEntities/">
	<!ENTITY fibo-be-fctx-sta "https://spec.edmcouncil.org/fibo/ontology/BE/FunctionalEntitiesExt/StateEntities/">
	<!ENTITY fibo-be-le-lp "https://spec.edmcouncil.org/fibo/ontology/BE/LegalEntities/LegalPersons/">
	<!ENTITY fibo-fnd-rel-rel "https://spec.edmcouncil.org/fibo/ontology/FND/Relations/Relations/">
	<!ENTITY fibo-fnd-utl-av "https://spec.edmcouncil.org/fibo/ontology/FND/Utilities/AnnotationVocabulary/">
	<!ENTITY owl "http://www.w3.org/2002/07/owl#">
	<!ENTITY rdf "http://www.w3.org/1999/02/22-rdf-syntax-ns#">
	<!ENTITY rdfs "http://www.w3.org/2000/01/rdf-schema#">
	<!ENTITY skos "http://www.w3.org/2004/02/skos/core#">
	<!ENTITY xsd "http://www.w3.org/2001/XMLSchema#">
]>
<rdf:RDF xml:base="https://spec.edmcouncil.org/fibo/ontology/BE/FunctionalEntitiesExt/StateEntities/"
	xmlns:dct="http://purl.org/dc/terms/"
	xmlns:fibo-be-fct-fct="https://spec.edmcouncil.org/fibo/ontology/BE/FunctionalEntities/FunctionalEntities/"
	xmlns:fibo-be-fctx-sta="https://spec.edmcouncil.org/fibo/ontology/BE/FunctionalEntitiesExt/StateEntities/"
	xmlns:fibo-be-le-lp="https://spec.edmcouncil.org/fibo/ontology/BE/LegalEntities/LegalPersons/"
	xmlns:fibo-fnd-rel-rel="https://spec.edmcouncil.org/fibo/ontology/FND/Relations/Relations/"
	xmlns:fibo-fnd-utl-av="https://spec.edmcouncil.org/fibo/ontology/FND/Utilities/AnnotationVocabulary/"
	xmlns:owl="http://www.w3.org/2002/07/owl#"
	xmlns:rdf="http://www.w3.org/1999/02/22-rdf-syntax-ns#"
	xmlns:rdfs="http://www.w3.org/2000/01/rdf-schema#"
	xmlns:skos="http://www.w3.org/2004/02/skos/core#"
	xmlns:xsd="http://www.w3.org/2001/XMLSchema#">
	
	<owl:Ontology rdf:about="https://spec.edmcouncil.org/fibo/ontology/BE/FunctionalEntitiesExt/StateEntities/">
		<rdfs:label xml:lang="en">StateEntities</rdfs:label>
		<dct:abstract>Selected kinds of entity in the government space, described in functional terms regardless of the precise legal form that they may take. Most such entities are now described in Release ontologies, while this ontology retains two that have not yet been adopted - government mortgage agency and sovereign wealth fund.</dct:abstract>
		<owl:imports rdf:resource="https://spec.edmcouncil.org/fibo/ontology/BE/FunctionalEntities/FunctionalEntities/"/>
		<owl:imports rdf:resource="https://spec.edmcouncil.org/fibo/ontology/BE/LegalEntities/LegalPersons/"/>
		<owl:imports rdf:resource="https://spec.edmcouncil.org/fibo/ontology/FND/Relations/Relations/"/>
		<owl:imports rdf:resource="https://spec.edmcouncil.org/fibo/ontology/FND/Utilities/AnnotationVocabulary/"/>
		<owl:imports rdf:resource="https://spec.edmcouncil.org/fibo/ontology/SEC/Debt/AssetBackedSecurities/MortgageBackedSecurities/"/>
		<owl:versionIRI rdf:resource="https://spec.edmcouncil.org/fibo/ontology/BE/FunctionalEntitiesExt/StateEntities/"/>
		<fibo-fnd-utl-av:hasMaturityLevel rdf:resource="&fibo-fnd-utl-av;Informative"/>
	</owl:Ontology>
	
	<owl:Class rdf:about="&fibo-be-fctx-sta;GovernmentMortgageAgency">
		<rdfs:subClassOf rdf:resource="&fibo-be-fct-fct;FunctionalEntity"/>
		<rdfs:subClassOf>
			<owl:Restriction>
				<owl:onProperty rdf:resource="&fibo-fnd-rel-rel;hasIdentity"/>
				<owl:someValuesFrom rdf:resource="&fibo-be-le-lp;LegalEntity"/>
			</owl:Restriction>
		</rdfs:subClassOf>
		<rdfs:label xml:lang="en">government mortgage agency</rdfs:label>
		<skos:definition xml:lang="en">An agency set up by a government for the purpose of issuing mortgages.</skos:definition>
		<skos:editorialNote xml:lang="en">Note on the original property &apos;takes form of&apos;  (replaced by a restriction): The form which the Government Mortgage Agency takes. This is a Legal Entity and not a Natural Person, that is, it is an Artificial Person.</skos:editorialNote>
		<skos:scopeNote xml:lang="en">These exist in the USA and may also exist now or in future in other countries. There are three such agencies in thr USA: FNMA, GNMA and FHLMC (Fannie Mae, Ginnie Mae and Freddie Mac respectively).</skos:scopeNote>
	</owl:Class>
	
	<owl:Class rdf:about="&fibo-be-fctx-sta;SovereignWealthFund">
		<rdfs:subClassOf rdf:resource="&fibo-be-fct-fct;FunctionalBusinessEntity"/>
		<rdfs:label xml:lang="en">sovereign wealth fund</rdfs:label>
		<skos:definition xml:lang="en">Government investment fund funded by foreign currency reserves. Review: Also include things like International Monetary Fund. Are these a Legal Entity? See also Funds model. Move the question about Sovereign Wealth Funds to the Funds model. Looking at definitions (e.g. Wikipedia) it&apos;s a state owned investment fund. The legal entity owner is a government (or in fact a State, which is governed by a Government).</skos:definition>
	</owl:Class>
	
	<owl:DatatypeProperty rdf:about="&fibo-be-fctx-sta;legalName">
		<rdfs:label xml:lang="en">legal name</rdfs:label>
	</owl:DatatypeProperty>

</rdf:RDF>