<?xml version="1.0" encoding="UTF-8"?>
<!DOCTYPE rdf:RDF [
	<!ENTITY fibo-be-fct-fct "https://spec.edmcouncil.org/fibo/BE/FunctionalEntities/FunctionalEntities/">
	<!ENTITY fibo-be-fctx-sta "https://spec.edmcouncil.org/fibo/BE/FunctionalEntitiesExt/StateEntities/">
	<!ENTITY fibo-be-le-lp "https://spec.edmcouncil.org/fibo/BE/LegalEntities/LegalPersons/">
	<!ENTITY fibo-fnd-rel-rel "https://spec.edmcouncil.org/fibo/FND/Relations/Relations/">
	<!ENTITY fibo-fnd-utl-av "https://spec.edmcouncil.org/fibo/FND/Utilities/AnnotationVocabulary/">
	<!ENTITY fibo-sec-dbt-ab-mbs "https://spec.edmcouncil.org/fibo/SEC/Debt/AssetBacked/MortgageBackedSecurities/">
	<!ENTITY owl "http://www.w3.org/2002/07/owl#">
	<!ENTITY rdf "http://www.w3.org/1999/02/22-rdf-syntax-ns#">
	<!ENTITY rdfs "http://www.w3.org/2000/01/rdf-schema#">
	<!ENTITY skos "http://www.w3.org/2004/02/skos/core#">
	<!ENTITY xsd "http://www.w3.org/2001/XMLSchema#">
]>
<rdf:RDF xml:base="https://spec.edmcouncil.org/fibo/BE/FunctionalEntitiesExt/StateEntities/"
	xmlns:fibo-be-fct-fct="https://spec.edmcouncil.org/fibo/BE/FunctionalEntities/FunctionalEntities/"
	xmlns:fibo-be-fctx-sta="https://spec.edmcouncil.org/fibo/BE/FunctionalEntitiesExt/StateEntities/"
	xmlns:fibo-be-le-lp="https://spec.edmcouncil.org/fibo/BE/LegalEntities/LegalPersons/"
	xmlns:fibo-fnd-rel-rel="https://spec.edmcouncil.org/fibo/FND/Relations/Relations/"
	xmlns:fibo-fnd-utl-av="https://spec.edmcouncil.org/fibo/FND/Utilities/AnnotationVocabulary/"
	xmlns:fibo-sec-dbt-ab-mbs="https://spec.edmcouncil.org/fibo/SEC/Debt/AssetBacked/MortgageBackedSecurities/"
	xmlns:owl="http://www.w3.org/2002/07/owl#"
	xmlns:rdf="http://www.w3.org/1999/02/22-rdf-syntax-ns#"
	xmlns:rdfs="http://www.w3.org/2000/01/rdf-schema#"
	xmlns:skos="http://www.w3.org/2004/02/skos/core#"
	xmlns:xsd="http://www.w3.org/2001/XMLSchema#">
	
	<owl:Ontology rdf:about="https://spec.edmcouncil.org/fibo/BE/FunctionalEntitiesExt/StateEntities/">
		<rdfs:label xml:lang="en">StateEntities</rdfs:label>
		<owl:imports rdf:resource="http://www.w3.org/2004/02/skos/core"/>
		<owl:imports rdf:resource="https://spec.edmcouncil.org/fibo/BE/FunctionalEntities/FunctionalEntities/"/>
		<owl:imports rdf:resource="https://spec.edmcouncil.org/fibo/BE/LegalEntities/LegalPersons/"/>
		<owl:imports rdf:resource="https://spec.edmcouncil.org/fibo/FND/Relations/Relations/"/>
		<owl:imports rdf:resource="https://spec.edmcouncil.org/fibo/FND/Utilities/AnnotationVocabulary/"/>
		<owl:imports rdf:resource="https://spec.edmcouncil.org/fibo/SEC/Debt/AssetBacked/MortgageBackedSecurities/"/>
		<fibo-fnd-utl-av:hasMaturityLevel rdf:resource="&fibo-fnd-utl-av;Informative"/>
	</owl:Ontology>
	
	<owl:Class rdf:about="&fibo-be-fctx-sta;GovernmentMortgageAgency">
		<rdfs:subClassOf rdf:resource="&fibo-be-fct-fct;FunctionalEntity"/>
		<rdfs:subClassOf>
			<owl:Restriction>
				<owl:onProperty rdf:resource="&fibo-fnd-rel-rel;hasIdentity"/>
				<owl:someValuesFrom rdf:resource="&fibo-be-le-lp;JuridicalPerson"/>
			</owl:Restriction>
		</rdfs:subClassOf>
		<rdfs:label xml:lang="en">government mortgage agency</rdfs:label>
		<skos:definition xml:lang="en">An agency set up by a government for the purpose of issuing mortgages.</skos:definition>
		<skos:editorialNote xml:lang="en">Note on the original property &apos;takes form of&apos;  (replaced by a restriction): The form which the Government Mortgage Agency takes. This is a Legal Entity and not a Natural Person, that is, it is an Artificial Person.</skos:editorialNote>
		<skos:scopeNote xml:lang="en">These exist in the USA and may also exist now or in future in other countries. There are three such agencies in thr USA: FNMA, GNMA and FHLMC (Fannie Mae, Ginnie Mae and Freddie Mac respectively).</skos:scopeNote>
	</owl:Class>
	
	<owl:Class rdf:about="&fibo-be-fctx-sta;SovereignWealthFund">
		<rdfs:subClassOf rdf:resource="&fibo-be-fct-fct;FunctionalBusinessEntity"/>
		<rdfs:label xml:lang="en">sovereign wealth fund</rdfs:label>
		<skos:definition xml:lang="en">Government investment fund funded by foreign currency reserves. Review: Also include things like International Monetary Fund. Are these a Legal Entity? See also Funds model. Move the question about Sovereign Wealth Funds to the Funds model. Looking at definitions (e.g. Wikipedia) it&apos;s a state owned investment fund. The legal entity owner is a government (or in fact a State, which is governed by a Government).</skos:definition>
	</owl:Class>
	
	<owl:DatatypeProperty rdf:about="&fibo-be-fctx-sta;legalName">
		<rdfs:label xml:lang="en">legal name</rdfs:label>
	</owl:DatatypeProperty>

</rdf:RDF>