<?xml version="1.0" encoding="UTF-8"?>
<!DOCTYPE rdf:RDF [
	<!ENTITY dct "http://purl.org/dc/terms/">
	<!ENTITY fibo-fbc-dae-crt "https://spec.edmcouncil.org/fibo/ontology/FBC/DebtAndEquities/CreditRatings/">
	<!ENTITY fibo-fbc-fi-fi "https://spec.edmcouncil.org/fibo/ontology/FBC/FinancialInstruments/FinancialInstruments/">
	<!ENTITY fibo-fnd-arr-cls "https://spec.edmcouncil.org/fibo/ontology/FND/Arrangements/ClassificationSchemes/">
	<!ENTITY fibo-fnd-arr-rt "https://spec.edmcouncil.org/fibo/ontology/FND/Arrangements/Ratings/">
	<!ENTITY fibo-fnd-org-fm "https://spec.edmcouncil.org/fibo/ontology/FND/Organizations/FormalOrganizations/">
	<!ENTITY fibo-fnd-rel-rel "https://spec.edmcouncil.org/fibo/ontology/FND/Relations/Relations/">
	<!ENTITY fibo-fnd-utl-av "https://spec.edmcouncil.org/fibo/ontology/FND/Utilities/AnnotationVocabulary/">
	<!ENTITY fibo-sec-sec-iss "https://spec.edmcouncil.org/fibo/ontology/SEC/Securities/SecuritiesIssuance/">
	<!ENTITY owl "http://www.w3.org/2002/07/owl#">
	<!ENTITY rdf "http://www.w3.org/1999/02/22-rdf-syntax-ns#">
	<!ENTITY rdfs "http://www.w3.org/2000/01/rdf-schema#">
	<!ENTITY skos "http://www.w3.org/2004/02/skos/core#">
	<!ENTITY xsd "http://www.w3.org/2001/XMLSchema#">
]>
<rdf:RDF xml:base="https://spec.edmcouncil.org/fibo/ontology/FBC/DebtAndEquities/CreditRatings/"
	xmlns:dct="http://purl.org/dc/terms/"
	xmlns:fibo-fbc-dae-crt="https://spec.edmcouncil.org/fibo/ontology/FBC/DebtAndEquities/CreditRatings/"
	xmlns:fibo-fbc-fi-fi="https://spec.edmcouncil.org/fibo/ontology/FBC/FinancialInstruments/FinancialInstruments/"
	xmlns:fibo-fnd-arr-cls="https://spec.edmcouncil.org/fibo/ontology/FND/Arrangements/ClassificationSchemes/"
	xmlns:fibo-fnd-arr-rt="https://spec.edmcouncil.org/fibo/ontology/FND/Arrangements/Ratings/"
	xmlns:fibo-fnd-org-fm="https://spec.edmcouncil.org/fibo/ontology/FND/Organizations/FormalOrganizations/"
	xmlns:fibo-fnd-rel-rel="https://spec.edmcouncil.org/fibo/ontology/FND/Relations/Relations/"
	xmlns:fibo-fnd-utl-av="https://spec.edmcouncil.org/fibo/ontology/FND/Utilities/AnnotationVocabulary/"
	xmlns:fibo-sec-sec-iss="https://spec.edmcouncil.org/fibo/ontology/SEC/Securities/SecuritiesIssuance/"
	xmlns:owl="http://www.w3.org/2002/07/owl#"
	xmlns:rdf="http://www.w3.org/1999/02/22-rdf-syntax-ns#"
	xmlns:rdfs="http://www.w3.org/2000/01/rdf-schema#"
	xmlns:skos="http://www.w3.org/2004/02/skos/core#"
	xmlns:xsd="http://www.w3.org/2001/XMLSchema#">
	
	<owl:Ontology rdf:about="https://spec.edmcouncil.org/fibo/ontology/FBC/DebtAndEquities/CreditRatings/">
		<rdfs:label xml:lang="en">Credit Ratings Ontology</rdfs:label>
		<dct:abstract>This ontology defines the concept of a credit rating, along with credit watch and outlook qualifying terms. There are credit ratings for individuals, for organizations and for instruments. 
		These are referenced extensively in the securities models but are also applicable to business entities generally and in the context of lending and account maintenance.</dct:abstract>
		<owl:imports rdf:resource="https://spec.edmcouncil.org/fibo/ontology/FBC/FinancialInstruments/FinancialInstruments/"/>
		<owl:imports rdf:resource="https://spec.edmcouncil.org/fibo/ontology/FND/Arrangements/ClassificationSchemes/"/>
		<owl:imports rdf:resource="https://spec.edmcouncil.org/fibo/ontology/FND/Arrangements/Ratings/"/>
		<owl:imports rdf:resource="https://spec.edmcouncil.org/fibo/ontology/FND/Organizations/FormalOrganizations/"/>
		<owl:imports rdf:resource="https://spec.edmcouncil.org/fibo/ontology/FND/Relations/Relations/"/>
		<owl:imports rdf:resource="https://spec.edmcouncil.org/fibo/ontology/FND/Utilities/AnnotationVocabulary/"/>
		<owl:versionIRI rdf:resource="https://spec.edmcouncil.org/fibo/ontology/FBC/DebtAndEquities/CreditRatings/"/>
		<fibo-fnd-utl-av:hasMaturityLevel rdf:resource="&fibo-fnd-utl-av;Provisional"/>
	</owl:Ontology>
	
	<owl:Class rdf:about="&fibo-fbc-dae-crt;CreditRating">
		<rdfs:subClassOf rdf:resource="&fibo-fnd-arr-rt;Rating"/>
		<rdfs:subClassOf>
			<owl:Restriction>
				<owl:onProperty rdf:resource="&fibo-fnd-rel-rel;isDefinedIn"/>
				<owl:someValuesFrom rdf:resource="&fibo-fbc-dae-crt;CreditRatingScale"/>
			</owl:Restriction>
		</rdfs:subClassOf>
		<rdfs:subClassOf>
			<owl:Restriction>
				<owl:onProperty rdf:resource="&fibo-fnd-rel-rel;isIssuedBy"/>
				<owl:someValuesFrom rdf:resource="&fibo-fbc-dae-crt;CreditRatingAgency"/>
			</owl:Restriction>
		</rdfs:subClassOf>
		<rdfs:label xml:lang="en">credit rating</rdfs:label>
		<skos:definition xml:lang="en">an assessment of creditworthiness of a borrower generally or with respect to a particular debt or financial obligation</skos:definition>
		<fibo-fnd-utl-av:explanatoryNote xml:lang="en">Typically, a credit rating is provided as a detailed report based on the financial history of borrowing or lending and creditworthiness of the entity or person derived from income statements, historical records related to borrowing, etc. with an aim to determine their ability to meet debt obligations.</fibo-fnd-utl-av:explanatoryNote>
	</owl:Class>
	
	<owl:Class rdf:about="&fibo-fbc-dae-crt;CreditRatingAgency">
		<rdfs:subClassOf rdf:resource="&fibo-fnd-arr-rt;RatingAgency"/>
		<rdfs:subClassOf>
			<owl:Restriction>
				<owl:onProperty rdf:resource="&fibo-fnd-rel-rel;issues"/>
				<owl:someValuesFrom rdf:resource="&fibo-fbc-dae-crt;CreditRating"/>
			</owl:Restriction>
		</rdfs:subClassOf>
		<rdfs:subClassOf>
			<owl:Restriction>
				<owl:onProperty rdf:resource="&fibo-fnd-rel-rel;manages"/>
				<owl:someValuesFrom rdf:resource="&fibo-fbc-dae-crt;CreditRatingScale"/>
			</owl:Restriction>
		</rdfs:subClassOf>
		<rdfs:label xml:lang="en">credit rating agency</rdfs:label>
		<skos:definition xml:lang="en">a rating agency that publishes reports assessing the creditworthiness of a borrower or legal entity, either generally or with respect to a specific obligation</skos:definition>
	</owl:Class>
	
	<owl:Class rdf:about="&fibo-fbc-dae-crt;CreditRatingScale">
		<rdfs:subClassOf rdf:resource="&fibo-fnd-arr-rt;RatingScale"/>
		<rdfs:subClassOf>
			<owl:Restriction>
				<owl:onProperty rdf:resource="&fibo-fnd-rel-rel;isManagedBy"/>
				<owl:someValuesFrom rdf:resource="&fibo-fbc-dae-crt;CreditRatingAgency"/>
			</owl:Restriction>
		</rdfs:subClassOf>
		<rdfs:label xml:lang="en">credit rating scale</rdfs:label>
		<skos:definition xml:lang="en">rating scale for assigning a credit rating to individual, entity, or instrument, including defining a set of codes or numeric scores and indicating how an assessment that is assigned a score based on that scale means</skos:definition>
	</owl:Class>
	
	<owl:Class rdf:about="&fibo-fbc-dae-crt;CreditWatchDirection">
		<rdfs:subClassOf rdf:resource="&fibo-fnd-arr-cls;Classifier"/>
		<rdfs:label xml:lang="en">credit watch direction</rdfs:label>
	</owl:Class>
	
	<owl:Class rdf:about="&fibo-fbc-dae-crt;CreditWatchDowngrade">
		<rdfs:subClassOf rdf:resource="&fibo-fbc-dae-crt;CreditWatchDirection"/>
		<rdfs:label xml:lang="en">credit watch downgrade</rdfs:label>
	</owl:Class>
	
	<owl:Class rdf:about="&fibo-fbc-dae-crt;CreditWatchOutlook">
		<rdfs:subClassOf rdf:resource="&fibo-fnd-arr-rt;Rating"/>
		<rdfs:label xml:lang="en">credit watch outlook</rdfs:label>
	</owl:Class>
	
	<owl:Class rdf:about="&fibo-fbc-dae-crt;CreditWatchUpgrade">
		<rdfs:subClassOf rdf:resource="&fibo-fbc-dae-crt;CreditWatchDirection"/>
		<rdfs:label xml:lang="en">credit watch upgrade</rdfs:label>
	</owl:Class>
	
	<owl:Class rdf:about="&fibo-fbc-dae-crt;IndividualCreditRating">
		<rdfs:subClassOf rdf:resource="&fibo-fbc-dae-crt;CreditRating"/>
		<rdfs:label xml:lang="en">individual credit rating</rdfs:label>
	</owl:Class>
	
	<owl:Class rdf:about="&fibo-fbc-dae-crt;InstrumentCreditRating">
		<rdfs:subClassOf rdf:resource="&fibo-fbc-dae-crt;InvestmentCreditRating"/>
		<rdfs:subClassOf>
			<owl:Restriction>
				<owl:onProperty rdf:resource="&fibo-fnd-arr-rt;rates"/>
				<owl:someValuesFrom rdf:resource="&fibo-fbc-fi-fi;FinancialInstrument"/>
			</owl:Restriction>
		</rdfs:subClassOf>
		<rdfs:label xml:lang="en">instrument credit rating</rdfs:label>
		<skos:definition xml:lang="en">An Instrument Credit Rating, that is the creditworthiness of the investment as determined by a Ratings Agency.</skos:definition>
		<fibo-fnd-utl-av:explanatoryNote xml:lang="en">For tranched securities: the instrument /is/ the Tranche for tranched securities so this is really just the Instrument Credit Rating under a different name? However the term Tranche Rating at Issue is meaningful.</fibo-fnd-utl-av:explanatoryNote>
	</owl:Class>
	
	<owl:Class rdf:about="&fibo-fbc-dae-crt;InvestmentCreditRating">
		<rdfs:subClassOf rdf:resource="&fibo-fbc-dae-crt;CreditRating"/>
		<rdfs:label xml:lang="en">investment credit rating</rdfs:label>
		<skos:definition xml:lang="en">The creditworthiness of an investment as determined by a Ratings Agency. Further notes: Anything can be bought and sold can have a rating. Credit rating can be assigned to an instrument, an organization, even a person. The rating is assigned to any kind of instrument that the organization etc. issues. Use Wikipedia credit rating definition Long term, short term and generic ratings The rating differentiates between short and long term (not sure about generic). In all systems these are differentiated. This relates to how long the holder might hold the thing. Or does it? The agencies offer two different servies and you pay 2 different fees for short and long. ACTION: to find The codes themselves are different. So it&apos;s not AAA etc. for short term it&apos;s something else. so the thing we&apos;ve been thinking about is actually long term ratings.</skos:definition>
	</owl:Class>
	
	<owl:Class rdf:about="&fibo-fbc-dae-crt;IssueCreditRating">
		<rdfs:subClassOf rdf:resource="&fibo-fbc-dae-crt;InvestmentCreditRating"/>
		<rdfs:label xml:lang="en">issue credit rating</rdfs:label>
		<skos:definition xml:lang="en">The creditworthiness of the overall issue as determined by a Ratings Agency.</skos:definition>
		<fibo-fnd-utl-av:explanatoryNote xml:lang="en">For a tranched secrutity issue, there is a credit rating for the overall issue as well as a different ratings for each tranche. The rating for the individual tranche is covered as the term &quot;Instrument Credit Rating&quot; since each tranche is an individual instrument (contract).</fibo-fnd-utl-av:explanatoryNote>
	</owl:Class>
	
	<owl:Class rdf:about="&fibo-fbc-dae-crt;OnWatchOutlook">
		<rdfs:subClassOf rdf:resource="&fibo-fbc-dae-crt;CreditWatchOutlook"/>
		<rdfs:label xml:lang="en">on watch outlook</rdfs:label>
	</owl:Class>
	
	<owl:Class rdf:about="&fibo-fbc-dae-crt;OrganizationCreditRating">
		<rdfs:subClassOf rdf:resource="&fibo-fbc-dae-crt;IndividualCreditRating"/>
		<rdfs:subClassOf>
			<owl:Restriction>
				<owl:onProperty rdf:resource="&fibo-fnd-arr-rt;rates"/>
				<owl:someValuesFrom rdf:resource="&fibo-fnd-org-fm;FormalOrganization"/>
			</owl:Restriction>
		</rdfs:subClassOf>
		<rdfs:label xml:lang="en">organization credit rating</rdfs:label>
		<skos:definition xml:lang="en">The credit rating of the organization. That is the creditworthiness of the organization as determined by a ratings agency. If the organization is the issuer of a security then this becomes the issuer rating for that security.</skos:definition>
	</owl:Class>
	
	<owl:Class rdf:about="&fibo-fbc-dae-crt;ShortTermCreditRating">
		<rdfs:subClassOf rdf:resource="&fibo-fbc-dae-crt;InvestmentCreditRating"/>
		<rdfs:label xml:lang="en">short term credit rating</rdfs:label>
		<skos:definition xml:lang="en">A short term rating is a probability factor of an individual going into default within a year. This is in contrast to long-term rating which is evaluated over a long timeframe.</skos:definition>
	</owl:Class>
	
	<owl:Class rdf:about="&fibo-fbc-dae-crt;StableOutlook">
		<rdfs:subClassOf rdf:resource="&fibo-fbc-dae-crt;CreditWatchOutlook"/>
		<rdfs:label xml:lang="en">stable outlook</rdfs:label>
	</owl:Class>
	
	<owl:ObjectProperty rdf:about="&fibo-fbc-dae-crt;watchDirection">
		<rdfs:label xml:lang="en">watch direction</rdfs:label>
		<rdfs:domain rdf:resource="&fibo-fbc-dae-crt;InvestmentCreditRating"/>
		<rdfs:range rdf:resource="&fibo-fbc-dae-crt;CreditWatchDirection"/>
		<skos:definition xml:lang="en">The direction in which the credit rating is expected to move, for something which has a credit rating on watch.</skos:definition>
	</owl:ObjectProperty>
	
	<owl:ObjectProperty rdf:about="&fibo-fbc-dae-crt;watchOutlook">
		<rdfs:label xml:lang="en">watch outlook</rdfs:label>
		<rdfs:domain rdf:resource="&fibo-fbc-dae-crt;InvestmentCreditRating"/>
		<rdfs:range rdf:resource="&fibo-fbc-dae-crt;CreditWatchOutlook"/>
		<skos:definition xml:lang="en">The expected outlook for the rated entity.</skos:definition>
	</owl:ObjectProperty>

</rdf:RDF>