<?xml version="1.0" encoding="UTF-8"?>
<!DOCTYPE rdf:RDF [
	<!ENTITY fibo-fbc-dae-crf "https://spec.edmcouncil.org/fibo/FBC/DebtAndEquities/CreditFacilities/">
	<!ENTITY fibo-fbc-dae-dbt "https://spec.edmcouncil.org/fibo/FBC/DebtAndEquities/Debt/">
	<!ENTITY fibo-fnd-agr-ctr "https://spec.edmcouncil.org/fibo/FND/Agreements/Contracts/">
	<!ENTITY fibo-fnd-agrx-con "https://spec.edmcouncil.org/fibo/FND/AgreementsExt/ContractualConstructs/">
	<!ENTITY fibo-fnd-pas-pas "https://spec.edmcouncil.org/fibo/FND/ProductsAndServices/ProductsAndServices/">
	<!ENTITY fibo-fnd-plc-fac "https://spec.edmcouncil.org/fibo/FND/Places/Facilities/">
	<!ENTITY fibo-fnd-rel-rel "https://spec.edmcouncil.org/fibo/FND/Relations/Relations/">
	<!ENTITY fibo-fnd-utl-av "https://spec.edmcouncil.org/fibo/FND/Utilities/AnnotationVocabulary/">
	<!ENTITY fibo-loan-loan-gen "https://spec.edmcouncil.org/fibo/LOAN/Loans/LoansGeneral/">
	<!ENTITY fibo-loan-loan-loan "https://spec.edmcouncil.org/fibo/LOAN/Loans/LoanBasicTerms/">
	<!ENTITY owl "http://www.w3.org/2002/07/owl#">
	<!ENTITY rdf "http://www.w3.org/1999/02/22-rdf-syntax-ns#">
	<!ENTITY rdfs "http://www.w3.org/2000/01/rdf-schema#">
	<!ENTITY skos "http://www.w3.org/2004/02/skos/core#">
	<!ENTITY xsd "http://www.w3.org/2001/XMLSchema#">
]>
<rdf:RDF xml:base="https://spec.edmcouncil.org/fibo/FBC/DebtAndEquities/CreditFacilities/"
	xmlns:fibo-fbc-dae-crf="https://spec.edmcouncil.org/fibo/FBC/DebtAndEquities/CreditFacilities/"
	xmlns:fibo-fbc-dae-dbt="https://spec.edmcouncil.org/fibo/FBC/DebtAndEquities/Debt/"
	xmlns:fibo-fnd-agr-ctr="https://spec.edmcouncil.org/fibo/FND/Agreements/Contracts/"
	xmlns:fibo-fnd-agrx-con="https://spec.edmcouncil.org/fibo/FND/AgreementsExt/ContractualConstructs/"
	xmlns:fibo-fnd-pas-pas="https://spec.edmcouncil.org/fibo/FND/ProductsAndServices/ProductsAndServices/"
	xmlns:fibo-fnd-plc-fac="https://spec.edmcouncil.org/fibo/FND/Places/Facilities/"
	xmlns:fibo-fnd-rel-rel="https://spec.edmcouncil.org/fibo/FND/Relations/Relations/"
	xmlns:fibo-fnd-utl-av="https://spec.edmcouncil.org/fibo/FND/Utilities/AnnotationVocabulary/"
	xmlns:fibo-loan-loan-gen="https://spec.edmcouncil.org/fibo/LOAN/Loans/LoansGeneral/"
	xmlns:fibo-loan-loan-loan="https://spec.edmcouncil.org/fibo/LOAN/Loans/LoanBasicTerms/"
	xmlns:owl="http://www.w3.org/2002/07/owl#"
	xmlns:rdf="http://www.w3.org/1999/02/22-rdf-syntax-ns#"
	xmlns:rdfs="http://www.w3.org/2000/01/rdf-schema#"
	xmlns:skos="http://www.w3.org/2004/02/skos/core#"
	xmlns:xsd="http://www.w3.org/2001/XMLSchema#">
	
	<owl:Ontology rdf:about="https://spec.edmcouncil.org/fibo/FBC/DebtAndEquities/CreditFacilities/">
		<rdfs:label xml:lang="en">CreditFacilities</rdfs:label>
		<owl:imports rdf:resource="http://www.w3.org/2004/02/skos/core"/>
		<owl:imports rdf:resource="https://spec.edmcouncil.org/fibo/FBC/DebtAndEquities/Debt/"/>
		<owl:imports rdf:resource="https://spec.edmcouncil.org/fibo/FND/Accounting/CurrencyAmount/"/>
		<owl:imports rdf:resource="https://spec.edmcouncil.org/fibo/FND/Agreements/Contracts/"/>
		<owl:imports rdf:resource="https://spec.edmcouncil.org/fibo/FND/AgreementsExt/ContractualConstructs/"/>
		<owl:imports rdf:resource="https://spec.edmcouncil.org/fibo/FND/Places/Facilities/"/>
		<owl:imports rdf:resource="https://spec.edmcouncil.org/fibo/FND/ProductsAndServices/ProductsAndServices/"/>
		<owl:imports rdf:resource="https://spec.edmcouncil.org/fibo/FND/Relations/Relations/"/>
		<owl:imports rdf:resource="https://spec.edmcouncil.org/fibo/FND/Utilities/AnnotationVocabulary/"/>
		<owl:imports rdf:resource="https://spec.edmcouncil.org/fibo/LOAN/Loans/LoanBasicTerms/"/>
		<owl:imports rdf:resource="https://spec.edmcouncil.org/fibo/LOAN/Loans/LoansGeneral/"/>
		<owl:versionIRI rdf:resource="https://spec.edmcouncil.org/fibo/FBC/DebtAndEquities/CreditFacilities/"/>
		<fibo-fnd-utl-av:hasMaturityLevel rdf:resource="&fibo-fnd-utl-av;Provisional"/>
	</owl:Ontology>
	
	<owl:Class rdf:about="&fibo-fbc-dae-crf;CommittedCreditFacility">
		<rdfs:subClassOf rdf:resource="&fibo-fbc-dae-crf;CreditFacility"/>
		<rdfs:subClassOf>
			<owl:Restriction>
				<owl:onProperty rdf:resource="&fibo-fbc-dae-crf;hasNegotated"/>
				<owl:someValuesFrom rdf:resource="&fibo-fbc-dae-crf;LendingCommitment"/>
			</owl:Restriction>
		</rdfs:subClassOf>
		<rdfs:label xml:lang="en">committed credit facility</rdfs:label>
		<owl:disjointWith rdf:resource="&fibo-fbc-dae-crf;UncommittedCreditFacility"/>
		<skos:definition xml:lang="en">A credit facility which has been formally agreed between a potential lender and a potential borrower.</skos:definition>
		<fibo-fnd-utl-av:explanatoryNote xml:lang="en">This represents a formal commitment from the potential lender. The commitment may also describe committed tranches of the Credit Facility set out for different purposes. This may have fees associated with it.</fibo-fnd-utl-av:explanatoryNote>
	</owl:Class>
	
	<owl:Class rdf:about="&fibo-fbc-dae-crf;CommittedCreditFacilityTranche">
		<rdfs:subClassOf rdf:resource="&fibo-fbc-dae-crf;CommittedCreditFacility"/>
		<rdfs:subClassOf rdf:resource="&fibo-fbc-dae-crf;CreditFacilityTranche"/>
		<rdfs:label xml:lang="en">committed credit facility tranche</rdfs:label>
		<owl:disjointWith rdf:resource="&fibo-fbc-dae-crf;UncommittedCreditFacilityTranche"/>
		<skos:definition xml:lang="en">A contractually committed line of credit which is issued as a revolving line of credit which can be drawn upon and has collateral</skos:definition>
		<skos:definition xml:lang="en">A tranche of a credit facility which has been formally agreed between a potential lender and a potential borrower.</skos:definition>
		<skos:editorialNote xml:lang="en">We now have it that all loans follow from a CommittedCredit Facility, but this may be transient. See notes on fees and Ts and Cs. See also FpML terms and elements on this. Apply to loan, draw-down generally (money market loan where we only see the actual lending). Is there also this feature in Money Markets, if you go straight to the market and they assess you on the spot? They have simply done the same kind of assessment. So maybe the concept of transient Cr facility tranche does not apply in that instance. There need be no firm commitment until the instrument is bought off you, at which point you have the capital. So this is where money markets and loans part company. Lending departments: create facility Money markets: deliver the money.</skos:editorialNote>
	</owl:Class>
	
	<owl:Class rdf:about="&fibo-fbc-dae-crf;CreditAgreementTerms">
		<rdfs:subClassOf rdf:resource="&fibo-fnd-agr-ctr;ContractualCommitment"/>
		<rdfs:label xml:lang="en">credit agremeent terms set</rdfs:label>
		<skos:definition xml:lang="en">Terms relating to an agreement to extend some committed credit facility on the part of a potential lender to a potential borrower.</skos:definition>
		<skos:editorialNote xml:lang="en">Includes terms for construction loans and other agreements which, while labeled as loans, are agreements to make loan advances at certain times and under certain conditions in the future. ACTIONS: Still need to connect these terms together in the overall model for Construction Loans and the rest. For now, added this term to take care of detail terms sets that are otherwise orphans. 14 July: What form does the set of terms of the commitment take? - will define a set of parameters or limits under which you are prepared to lend money. These may include: Pledges, negative pledges; pledge of security that is available to you if you lend the loan/ also restrictions on how frequently the tranche can be drawn down whether or under what conditions you can re-draw. These terms will determine the nature of the loan. so for example a student loan will have quite a restrictive facility. The facility probably on&apos;t just pay you money, it may for instance pay against a receipt for the fees, or may pay the institution directly. These terms are designed to control the credit risk that the lender (or ultimate lender) is going to take. Also you are charged for providing that facility - the bank, once it&apos;s made that commitment, will have had to set aside capital. They have no control of when you are going to draw down on that loan, so the bank has to ensure that when you do they don&apos;t exceed their capital requirements. There is a fee to cover this. Syndicated lending is more complex - there would be multiple lenders when the draw-down takes place - the potential lenders are numerous, and will be beyond the credit limits of any individual bank. these have agents, managers and so on, as well as the syndicate members who participate in the lending. Manager: does all the organization. calls people (lenders) together when the borrower makes a draw down, and distributes this. See Syndicate Loan diagram. This can be turned into multiple actual loans. There would be separate limits in these, based on currency, risk type and so on (as per Credit Facility generally). So one might use the borrowing for trade finance, revolving credit facility, straight draw-down, all specified in terms of the limits (maximum amounts that the lenders are prepared to give). A facility may also be a stand-by facility - one you may never want to draw down but need as protection.</skos:editorialNote>
	</owl:Class>
	
	<owl:Class rdf:about="&fibo-fbc-dae-crf;CreditExtension">
		<rdfs:subClassOf rdf:resource="&fibo-fnd-pas-pas;Service"/>
		<rdfs:label xml:lang="en">credit extension</rdfs:label>
		<skos:definition xml:lang="en">A service whereby credit is extended from the service provider to some party i.e. a borrower.</skos:definition>
	</owl:Class>
	
	<owl:Class rdf:about="&fibo-fbc-dae-crf;CreditFacility">
		<rdfs:subClassOf rdf:resource="&fibo-fnd-plc-fac;Facility"/>
		<rdfs:subClassOf>
			<owl:Restriction>
				<owl:onProperty rdf:resource="&fibo-fbc-dae-crf;hasTranche"/>
				<owl:someValuesFrom rdf:resource="&fibo-fbc-dae-crf;CreditFacilityTranche"/>
			</owl:Restriction>
		</rdfs:subClassOf>
		<rdfs:label xml:lang="en">credit facility</rdfs:label>
		<skos:definition xml:lang="en">An option to borrow money. Defines the parameters in which you are able to draw down some amount as a loan, debt finance, or some other financial commitment.</skos:definition>
		<skos:editorialNote xml:lang="en">There may also be min and max parcels of these. May also be fees for this facility. Review Questions and Discussion: QUESTION: Are there significant meaningful differences between retail and corporate? In the corporate world you may sit down and make an agreement between the lender and the potential borrower, to agreement. Corporate: Committed lending v Uncommitted lending. Sets limits what they are prepared to lend to a customer but don&apos;t make an agreement with the customer. Separately: May go into a &quot;Specified Commitment&quot; to make that lending. We say to the customer we are prepared to lend you x amount and of that, we will say, that eg 100M can be drawn down in this way, e.g as a direct loan, another 100M may be in terms of guarantees offered. May also put a lot of structure around how that may be drawn. Project financing / construction finance is where we have limits about this. You are constructing your own collateral in the construction. The collateral is an agreement where you may size these assets in the event of a default. Collateral may be associatedd irectly with the loan OR directly with the Facility. In the latter case you would not have to renegotiate collateral agreements every time you draw down on that loan. How this works: The Credit Facility in this latter case, is a bilateral contract: The lender is legally committing to be able to extend that amount of money. Borrower can borrow (or not) as and when they see fit. The lender has to then set aside capital for that money. It is now the borrower&apos;s right to determine when and how they draw this. So the central facility says we would do those loans - within the context for that facility. In retail:: there is no flexibility to negotiate, the Ts &amp; Cs are fairly standard. All the above concepts still exist in retail. So bank has limit they are prepared to lend that customer., determined in the context of the amount of collateral the retail customer can provide. Can still have construction loans in retail lending. See also syndicated loans. Set up with panel of potential vendors.</skos:editorialNote>
		<skos:editorialNote xml:lang="en">We now have it that all loans follow from a CommittedCredit Facility, but this may be transient. See notes on fees and Ts and Cs. See also FpML terms and elements on this. Apply to loan, draw-down generally (money market loan where we only see the actual lending). Is there also this feature in Money Markets, if you go straight to the market and they assess you on the spot? They have simply done the same kind of assessment. So maybe the concept of transient Cr facility tranche does not apply in that instance. There need be no firm commitment until the instrument is bought off you, at which point you have the capital. So this is where money markets and loans part company. Lending departments: create facility Money markets: deliver the money.</skos:editorialNote>
	</owl:Class>
	
	<owl:Class rdf:about="&fibo-fbc-dae-crf;CreditFacilityAgreement">
		<rdfs:subClassOf rdf:resource="&fibo-fnd-agr-ctr;MutualContractualAgreement"/>
		<rdfs:subClassOf rdf:resource="&fibo-fnd-agr-ctr;WrittenContract"/>
		<rdfs:subClassOf>
			<owl:Restriction>
				<owl:onProperty rdf:resource="&fibo-fbc-dae-crf;setsOutCommitmentTo"/>
				<owl:someValuesFrom rdf:resource="&fibo-fbc-dae-crf;CommittedCreditFacility"/>
			</owl:Restriction>
		</rdfs:subClassOf>
		<rdfs:subClassOf>
			<owl:Restriction>
				<owl:onProperty rdf:resource="&fibo-fnd-agr-ctr;hasContractualElement"/>
				<owl:someValuesFrom rdf:resource="&fibo-fbc-dae-crf;CreditAgreementTerms"/>
			</owl:Restriction>
		</rdfs:subClassOf>
		<rdfs:subClassOf>
			<owl:Restriction>
				<owl:onProperty rdf:resource="&fibo-fnd-agr-ctr;hasContractualElement"/>
				<owl:someValuesFrom rdf:resource="&fibo-fbc-dae-crf;LoanPrecedentConditions"/>
			</owl:Restriction>
		</rdfs:subClassOf>
		<rdfs:subClassOf>
			<owl:Restriction>
				<owl:onProperty rdf:resource="&fibo-fnd-agrx-con;mandates"/>
				<owl:someValuesFrom rdf:resource="&fibo-fbc-dae-crf;LendingCommitment"/>
			</owl:Restriction>
		</rdfs:subClassOf>
		<rdfs:label xml:lang="en">credit facility agreement</rdfs:label>
		<skos:definition xml:lang="en">A formal contract in which a potential lender agrees to lend to a potential borrower under terms stated in this contract.</skos:definition>
		<fibo-fnd-utl-av:explanatoryNote xml:lang="en">The agreement will usually also define tranches of the credit facility to which they are prepared to commit lending for specific purposes. Note that the existence of this formal agreement represents a fornal commmitment by the potential lender. This results in formal provisions needing to be made in terms of the lender&apos;s overall positions and exposures. See new notes in Credit Facility and elsewhere. These define the terms that belong in this box. Upper ontology: abstract so that every loan starts off as a credit facility. Then it should all fall into place.</fibo-fnd-utl-av:explanatoryNote>
	</owl:Class>
	
	<owl:Class rdf:about="&fibo-fbc-dae-crf;CreditFacilityGuarantyTranche">
		<rdfs:subClassOf rdf:resource="&fibo-fbc-dae-crf;CreditFacilityTranche"/>
		<rdfs:subClassOf>
			<owl:Restriction>
				<owl:onProperty rdf:resource="&fibo-fbc-dae-crf;hasTranchePurpose"/>
				<owl:someValuesFrom rdf:resource="&fibo-fbc-dae-crf;CreditFacilityTypeSelection"/>
			</owl:Restriction>
		</rdfs:subClassOf>
		<rdfs:label xml:lang="en">credit facility guaranty tranche</rdfs:label>
		<owl:disjointWith rdf:resource="&fibo-fbc-dae-crf;CreditFacilityLoanTranche"/>
		<owl:disjointWith rdf:resource="&fibo-fbc-dae-crf;CreditFacilitySecuritiesTranche"/>
	</owl:Class>
	
	<owl:Class rdf:about="&fibo-fbc-dae-crf;CreditFacilityLoanTranche">
		<rdfs:subClassOf rdf:resource="&fibo-fbc-dae-crf;CreditFacilityTranche"/>
		<rdfs:subClassOf>
			<owl:Restriction>
				<owl:onProperty rdf:resource="&fibo-fbc-dae-crf;hasTranchePurpose"/>
				<owl:someValuesFrom rdf:resource="&fibo-fbc-dae-crf;CreditFacilityTypeSelection"/>
			</owl:Restriction>
		</rdfs:subClassOf>
		<rdfs:subClassOf>
			<owl:Restriction>
				<owl:onProperty rdf:resource="&fibo-fbc-dae-crf;issuedAs"/>
				<owl:someValuesFrom rdf:resource="&fibo-loan-loan-loan;LoanDrawdown"/>
			</owl:Restriction>
		</rdfs:subClassOf>
		<rdfs:label xml:lang="en">credit facility loan tranche</rdfs:label>
		<owl:disjointWith rdf:resource="&fibo-fbc-dae-crf;CreditFacilitySecuritiesTranche"/>
		<skos:definition xml:lang="en">A tranche of a credit facility the purpose of which is a kind of Loan.</skos:definition>
	</owl:Class>
	
	<owl:Class rdf:about="&fibo-fbc-dae-crf;CreditFacilitySecuritiesTranche">
		<rdfs:subClassOf rdf:resource="&fibo-fbc-dae-crf;CreditFacilityTranche"/>
		<rdfs:subClassOf>
			<owl:Restriction>
				<owl:onProperty rdf:resource="&fibo-fbc-dae-crf;hasTranchePurpose"/>
				<owl:someValuesFrom rdf:resource="&fibo-fbc-dae-crf;CreditFacilityTypeSelection"/>
			</owl:Restriction>
		</rdfs:subClassOf>
		<rdfs:subClassOf>
			<owl:Restriction>
				<owl:onProperty rdf:resource="&fibo-fbc-dae-crf;issuedAs"/>
				<owl:someValuesFrom rdf:resource="&fibo-loan-loan-gen;UnsubscribedDebt"/>
			</owl:Restriction>
		</rdfs:subClassOf>
		<rdfs:label xml:lang="en">credit facility securities tranche</rdfs:label>
	</owl:Class>
	
	<owl:Class rdf:about="&fibo-fbc-dae-crf;CreditFacilityTranche">
		<rdfs:subClassOf rdf:resource="&fibo-fbc-dae-crf;CreditFacility"/>
		<rdfs:label xml:lang="en">credit facility tranche</rdfs:label>
		<skos:definition xml:lang="en">An individual tranche of the Credit Facility. This is the maximal amount of credit that can be extended to the potential borrower for the stated purpose.</skos:definition>
		<fibo-fnd-utl-av:explanatoryNote xml:lang="en">The amount of each tranche of the credit facility sums to the total Credit Facility amount. Tranches of the Credit Facility each have a stated purpose. Credit Facility may includes provision of loans, of guarantees, credit finance and other things that can create a credit exposure. Scope of Credit Facility Tranches: Many tranches are for loans. For retail borrowers these would be the only types of tranche. For other types of potential borrowers e.g. corporates, other tranches of credit facility may include for securitized debt (where the potential borrower is a corporation), or for guaranty provision. (detailed note from SME Review 10 Feb 2011) Credit Facility may also have provision of guarantees, credit finance and other things that can create a credit exposure. These are all in the Credit Facility Tranche. Sets terms under which the lender may make a number of tns which may create the redit risk. The tranche may be the creation of the credit risk See also CDO, where the Pf is structured in a way that might then be subject to these considerations. Not the same meaning as Tranches in CDOs. (note ends) PoC (2010) notes (specific to Loan trahche) Note that since this time the scope of these has been extended since credit facility is also relevant to securitized debt, and other cretid exposures (guaranty etc.). The amount of each tranche, summed up. makes up the Credit Facillity amount. Each tranche has a loan type. One or more loans are issued against this transhe Against the loan will be one or more draw downs. Example: Take a tranche for Credit Line. This is $300K. against that $300K tranche, I issue a credit line loan of $200K . Against that loan of $200K I may draw $10K An amount you are good for under agreed termas and conditions. A credit line is not necessarily going to be drawn. Drawn is the Current debt obligation and may change from day to day. Simpler example: Construction Loan Credit Facility of $1M for this person Against a tranche of Construction Loan, I can have $300 tranche of credit facility. NOT A LOAN. Against that tranche of $300K I can create a loan (take a loan) for Construction, of $200K. That loan is also going to be advanced in several draw-downs. Once I complete the 1st phase of construction, for example at the start I get an initial 10$ for a draw of 15K, then after the 1st phase I get a draw of another 15% and so on. That is where debt and loan differ because the debt is what you are paying interest on (the outstanding balance) which reflects a cumulative sum of draw minus any principal repayments. The difference between these is to be explained at a future session. A given tranche will observe all of the requirements of a credit facility. It has additional requirements. So a Credit Facility has multiple tranches. It does not inherit Amount. Credit Facility Amounts are distinct from Tranche Amount. 14 July: Credit Faciliy versus Committed Credit Facility. Recall that a non committe credit facility implies no commitment on the part of the potential lender. Once they are committed to it, that&apos;s a contractual commitment. However, before they do that, they assess your credit (and/or collateral or other forms of interest). What happens as time goes along? There are Ts and Cs in the facility, including a termination date (and general temrination clauses). Are there general termination clauses for instance for changes to circumstances? there is an Evergreen concept, whereby the(potential) lender has the right to revise the Ts and Cs, and terminate the loan, on a given, pre-stated review date. So the Evergreen term has conditions about what happens to outstanding loans and so on. the bank will structure lending to be able to get out as required, for example the loan may not go on beyond the Evergreen review date. This is not hard and fast though - the proviedr of the facility manages this and decides accordingly. May noe be all that obvious to the borrower what happens. Meanwhile, with revolving facility there is by definitoin a review date. Modeling: Add these (Evergreen) etc. terms to the terms for the committed credit facility. There might be conditions in the lending agreement that say how we will handle that. Are there terms i nthe Loan contract itself that refer back tot hese? Yes. The Loan Documentation will reference the Credit Facility. Compare with ISDA Master Agreement. Are there also Termination clases based on default events? (as per ISDA MA)? Most likely. These will be defined in the loan agreement. The pre-agreed terms, these are the Conditions Precedent (see elsewhere in the model) The Conditions Precedent are those things that have ot happen before the loan comes into play, for example stumping up collaterial, setting up ESCROW accounts and that kind of thing, that have to happen before the FACILITY comes into existence. So there are Conditions Precedent to the Facility, and Conditions Presedent to the Loan. So for instance negative pledges etc. - during the life of the loan you would have to confirm that you are in compliance with the conditions in the NEgative Pledge agreement. These will be Conditions Subsequent. Are there &quot;Conditions Precedent&quot; to the loan itself? Seemingly not. The loan is committed. for a non committed Credit Facility (e.g. general loan, auto loan, mortgage, lent to individuals), there are no Conditions Precedent because the bank either agrees the loan or they do not. Even for a single up front loan, there is in principle a Credit Facility which is immediately drawn down. So during that initial (intra day) period of time, there is a committed credit facility. So there is always a committed Credit Facility even if it&apos;s only transient before it is drawn down. So Credit Facility may be committed or not. but all loan are drawn down from Committed Credit Facility, even if that commitment is only transient i.e. the loan is dranw down right away. In this case, the commitment is discharged right away as a draw down. So the existence of a fee, only applies to committed credit facility tranches which are not transient. The &quot;fees&quot; as such are embedded in the interest rate. Whatever costs are incurred are passed right through as interest rate. Whereas, with credit facilitie that exist for a time, there are additional costs, and these are passed on as fees. This is the logic of having &quot;undrawn fees&quot;. Example: Overdraft facility has a fee, which even if you don&apos;t use the overdraft, they charge you an undrawn fee. At the bank&apos;s discretion they might not charge fo rhtis, but recover the costs elsewhere. They may also have restrictions on whether you can have it there unused and so on. Modeling: Can construct almost any of these in whatever combination. So make sure that the model bears this out. So going into the Credit Facility is: - credit checking - Collateral - Security Interest as a general term these are, in common, all &quot;Credit Control&quot; or credit min=tigation features. Guaranties are another. CDS is also a form of guaranty, where someone guarantees that the other party will pay. Or it may take the form of some ownership transfer (?) Default: activates a Credit Support Agreement. Default event triggers the credit support agreement between the lender and the potential borrower (or a third party - see Guaranty), describing what the borrower (por other party) says the lender can do in the event of default. See Credit Support Agreements as a whole - we should model these. Also relates to the posting of collateral in OTC swaps and the like. This is also where central counterparties provide a mechanism for centralizing the risk of these. The central agency is holding the securities that each party has posted in their Master Agreement with the central counterparty (e.g. clearing house). Guaranties create contagion.</fibo-fnd-utl-av:explanatoryNote>
	</owl:Class>
	
	<owl:Class rdf:about="&fibo-fbc-dae-crf;CreditFacilityTypeSelection">
		<rdfs:label xml:lang="en">CreditFacilityTypeSelection</rdfs:label>
		<skos:definition xml:lang="en">Types of purpose for which a credit facility tranche may be set up or may exist.</skos:definition>
	</owl:Class>
	
	<owl:Class rdf:about="&fibo-fbc-dae-crf;CreditProvider">
		<rdfs:subClassOf rdf:resource="&fibo-fnd-pas-pas;ServiceProvider"/>
		<rdfs:subClassOf>
			<owl:Restriction>
				<owl:onProperty rdf:resource="&fibo-fnd-rel-rel;provides"/>
				<owl:someValuesFrom rdf:resource="&fibo-fbc-dae-crf;CreditExtension"/>
			</owl:Restriction>
		</rdfs:subClassOf>
		<rdfs:label xml:lang="en">credit provider</rdfs:label>
	</owl:Class>
	
	<owl:Class rdf:about="&fibo-fbc-dae-crf;LendingCommitment">
		<rdfs:subClassOf rdf:resource="&fibo-fnd-agr-ctr;ContractualCommitment"/>
		<rdfs:label xml:lang="en">lending commitment</rdfs:label>
		<skos:definition xml:lang="en">Some commitment to enter into some lending arrangement at some point in the future.</skos:definition>
		<fibo-fnd-utl-av:explanatoryNote xml:lang="en">This commitment involves two (or more) parties: the party which makes a commitment to lend and the party or parties to which that commitment is made (and who thereby enjoy the corresponding right i.e. the expectation to be lent to under the terms defined in the or any contract which underpins and mechanizes this commitment).</fibo-fnd-utl-av:explanatoryNote>
	</owl:Class>
	
	<owl:Class rdf:about="&fibo-fbc-dae-crf;LoanPrecedentConditions">
		<rdfs:subClassOf rdf:resource="&fibo-fbc-dae-crf;CreditAgreementTerms"/>
		<rdfs:label xml:lang="en">loan precedent conditions</rdfs:label>
		<skos:definition xml:lang="en">Conditions which must be met before a loan may be approved.</skos:definition>
	</owl:Class>
	
	<owl:Class rdf:about="&fibo-fbc-dae-crf;UncommittedCreditFacility">
		<rdfs:subClassOf rdf:resource="&fibo-fbc-dae-crf;CreditFacility"/>
		<rdfs:label xml:lang="en">uncommitted credit facility</rdfs:label>
	</owl:Class>
	
	<owl:Class rdf:about="&fibo-fbc-dae-crf;UncommittedCreditFacilityTranche">
		<rdfs:subClassOf rdf:resource="&fibo-fbc-dae-crf;CreditFacilityTranche"/>
		<rdfs:subClassOf rdf:resource="&fibo-fbc-dae-crf;UncommittedCreditFacility"/>
		<rdfs:label xml:lang="en">uncommitted credit facility tranche</rdfs:label>
	</owl:Class>
	
	<owl:ObjectProperty rdf:about="&fibo-fbc-dae-crf;hasNegotated">
		<rdfs:label xml:lang="en">has negotiated</rdfs:label>
		<rdfs:domain rdf:resource="&fibo-fbc-dae-crf;CommittedCreditFacility"/>
		<rdfs:range rdf:resource="&fibo-fbc-dae-crf;LendingCommitment"/>
	</owl:ObjectProperty>
	
	<owl:ObjectProperty rdf:about="&fibo-fbc-dae-crf;hasTranche">
		<rdfs:subPropertyOf rdf:resource="&fibo-fnd-rel-rel;hasPart"/>
		<rdfs:label xml:lang="en">has tranche</rdfs:label>
		<rdfs:domain rdf:resource="&fibo-fbc-dae-crf;CreditFacility"/>
		<rdfs:range rdf:resource="&fibo-fbc-dae-crf;CreditFacilityTranche"/>
	</owl:ObjectProperty>
	
	<owl:ObjectProperty rdf:about="&fibo-fbc-dae-crf;hasTranchePurpose">
		<rdfs:label xml:lang="en">has tranche purpose</rdfs:label>
		<rdfs:domain rdf:resource="&fibo-fbc-dae-crf;CreditFacilityTranche"/>
		<rdfs:range rdf:resource="&fibo-fbc-dae-crf;CreditFacilityTypeSelection"/>
		<skos:definition xml:lang="en">The purpose for which the Tranche may exist. Notes 10 Feb: Question: What about a website that offers facilities for multiple purposes? Sometimes facility and purpose are not kept distinct. Differences: Retail lending - as modeled here commercial lending - see notes Purpose - Specific lenders e.g. Sallie Mae: Is it a loan or a credit facility? Is it structured similar to Construction / project loan? May look like multiple loans but these are fungible so it looks like one loan? Semantically: Facility v Loan? Student loan: usually for no more than one year. Would have multiple loans, so e.g. 2 or 3 semesters. School sets up number of disbursements so that tan equal amount goes at the start of a given semestrer. Next year you apply again for the loan AND before that you reassess the credit worthiness, so this means you are applying for a new Credit Facility Tranche as defined here. Always treated as a separate loan. School also has to certify that loan. See status - schol status, grace period status. Defer, small fixed, etc. versus full P&amp;I which applies when they have left school May be 10 years or so. Would be separate loans, but pulled into one bull group, with one payment. May be a min payment amount to be applied abgainst each loan, say min $50 per payment, based upon the Program. Is the Program a facility?? Or should we regard it as a kind of pool of loans, with a single repayment schedule. Account? Consolidation. The individual doesn&apos;t have to see loads of statements.</skos:definition>
	</owl:ObjectProperty>
	
	<owl:ObjectProperty rdf:about="&fibo-fbc-dae-crf;issuedAs">
		<rdfs:label xml:lang="en">issued as</rdfs:label>
		<rdfs:domain rdf:resource="&fibo-fbc-dae-crf;CreditFacilityTranche"/>
		<rdfs:range rdf:resource="&fibo-fbc-dae-dbt;Debt"/>
	</owl:ObjectProperty>
	
	<owl:ObjectProperty rdf:about="&fibo-fbc-dae-crf;setsOutCommitmentTo">
		<rdfs:label xml:lang="en">sets out commitment to</rdfs:label>
		<rdfs:domain rdf:resource="&fibo-fbc-dae-crf;CreditFacilityAgreement"/>
		<rdfs:range rdf:resource="&fibo-fbc-dae-crf;CommittedCreditFacility"/>
	</owl:ObjectProperty>
	
	<owl:ObjectProperty rdf:about="&fibo-fbc-dae-crf;trancheHasLoanPurpose">
		<rdfs:label xml:lang="en">tranche has loan purpose</rdfs:label>
		<rdfs:domain rdf:resource="&fibo-fbc-dae-crf;CreditFacilityLoanTranche"/>
		<rdfs:range rdf:resource="&fibo-loan-loan-loan;LoanPurposeSelection"/>
	</owl:ObjectProperty>
	
	<owl:DatatypeProperty rdf:about="&fibo-fbc-dae-crf;trancheLoanPurpose">
		<rdfs:label xml:lang="en">tranche loan purpose</rdfs:label>
	</owl:DatatypeProperty>

</rdf:RDF>