<?xml version="1.0" encoding="UTF-8"?>
<!DOCTYPE rdf:RDF [
	<!ENTITY dct "http://purl.org/dc/terms/">
	<!ENTITY fibo-be-le-cb "https://spec.edmcouncil.org/fibo/ontology/BE/LegalEntities/CorporateBodies/">
	<!ENTITY fibo-fbc-dae-cre "https://spec.edmcouncil.org/fibo/ontology/FBC/DebtAndEquities/CreditEvents/">
	<!ENTITY fibo-fbc-dae-dbt "https://spec.edmcouncil.org/fibo/ontology/FBC/DebtAndEquities/Debt/">
	<!ENTITY fibo-fnd-acc-cur "https://spec.edmcouncil.org/fibo/ontology/FND/Accounting/CurrencyAmount/">
	<!ENTITY fibo-fnd-dt-fd "https://spec.edmcouncil.org/fibo/ontology/FND/DatesAndTimes/FinancialDates/">
	<!ENTITY fibo-fnd-dt-oc "https://spec.edmcouncil.org/fibo/ontology/FND/DatesAndTimes/Occurrences/">
	<!ENTITY fibo-fnd-org-fm "https://spec.edmcouncil.org/fibo/ontology/FND/Organizations/FormalOrganizations/">
	<!ENTITY fibo-fnd-rel-rel "https://spec.edmcouncil.org/fibo/ontology/FND/Relations/Relations/">
	<!ENTITY fibo-fnd-utl-av "https://spec.edmcouncil.org/fibo/ontology/FND/Utilities/AnnotationVocabulary/">
	<!ENTITY owl "http://www.w3.org/2002/07/owl#">
	<!ENTITY rdf "http://www.w3.org/1999/02/22-rdf-syntax-ns#">
	<!ENTITY rdfs "http://www.w3.org/2000/01/rdf-schema#">
	<!ENTITY skos "http://www.w3.org/2004/02/skos/core#">
	<!ENTITY sm "http://www.omg.org/techprocess/ab/SpecificationMetadata/">
	<!ENTITY xsd "http://www.w3.org/2001/XMLSchema#">
]>
<rdf:RDF xml:base="https://spec.edmcouncil.org/fibo/ontology/FBC/DebtAndEquities/CreditEvents/"
	xmlns:dct="http://purl.org/dc/terms/"
	xmlns:fibo-be-le-cb="https://spec.edmcouncil.org/fibo/ontology/BE/LegalEntities/CorporateBodies/"
	xmlns:fibo-fbc-dae-cre="https://spec.edmcouncil.org/fibo/ontology/FBC/DebtAndEquities/CreditEvents/"
	xmlns:fibo-fbc-dae-dbt="https://spec.edmcouncil.org/fibo/ontology/FBC/DebtAndEquities/Debt/"
	xmlns:fibo-fnd-acc-cur="https://spec.edmcouncil.org/fibo/ontology/FND/Accounting/CurrencyAmount/"
	xmlns:fibo-fnd-dt-fd="https://spec.edmcouncil.org/fibo/ontology/FND/DatesAndTimes/FinancialDates/"
	xmlns:fibo-fnd-dt-oc="https://spec.edmcouncil.org/fibo/ontology/FND/DatesAndTimes/Occurrences/"
	xmlns:fibo-fnd-org-fm="https://spec.edmcouncil.org/fibo/ontology/FND/Organizations/FormalOrganizations/"
	xmlns:fibo-fnd-rel-rel="https://spec.edmcouncil.org/fibo/ontology/FND/Relations/Relations/"
	xmlns:fibo-fnd-utl-av="https://spec.edmcouncil.org/fibo/ontology/FND/Utilities/AnnotationVocabulary/"
	xmlns:owl="http://www.w3.org/2002/07/owl#"
	xmlns:rdf="http://www.w3.org/1999/02/22-rdf-syntax-ns#"
	xmlns:rdfs="http://www.w3.org/2000/01/rdf-schema#"
	xmlns:skos="http://www.w3.org/2004/02/skos/core#"
	xmlns:sm="http://www.omg.org/techprocess/ab/SpecificationMetadata/"
	xmlns:xsd="http://www.w3.org/2001/XMLSchema#">
	
	<owl:Ontology rdf:about="https://spec.edmcouncil.org/fibo/ontology/FBC/DebtAndEquities/CreditEvents/">
		<rdfs:label xml:lang="en">Credit Events Ontology</rdfs:label>
		<dct:abstract>This ontology defines a range of credit events, that is events in which some payment or payments are not made. These include credit events relating to a specific debt obligation and events relating to the business entity as a whole. 
		Note: these were derived from the credit default swaps model, with extensive reference to the FpML standard for those instruments. Additional kinds of credit event may be needed for loan and other contexts.</dct:abstract>
		<dct:license rdf:datatype="&xsd;anyURI">http://opensource.org/licenses/MIT</dct:license>
		<sm:contentLanguage rdf:datatype="&xsd;anyURI">http://www.w3.org/standards/techs/owl#w3c_all</sm:contentLanguage>
		<sm:copyright>Copyright (c) 2018-2019 EDM Council, Inc.</sm:copyright>
		<sm:dependsOn rdf:resource="https://spec.edmcouncil.org/fibo/ontology/BE/"/>
		<sm:dependsOn rdf:resource="https://spec.edmcouncil.org/fibo/ontology/FBC/DebtAndEquities/Debt/"/>
		<sm:dependsOn rdf:resource="https://spec.edmcouncil.org/fibo/ontology/FND/"/>
		<sm:fileAbbreviation>fibo-fbc-dae-cre</sm:fileAbbreviation>
		<sm:filename>CreditEvents.rdf</sm:filename>
		<owl:imports rdf:resource="https://spec.edmcouncil.org/fibo/ontology/BE/LegalEntities/CorporateBodies/"/>
		<owl:imports rdf:resource="https://spec.edmcouncil.org/fibo/ontology/FBC/DebtAndEquities/Debt/"/>
		<owl:imports rdf:resource="https://spec.edmcouncil.org/fibo/ontology/FND/Accounting/CurrencyAmount/"/>
		<owl:imports rdf:resource="https://spec.edmcouncil.org/fibo/ontology/FND/DatesAndTimes/FinancialDates/"/>
		<owl:imports rdf:resource="https://spec.edmcouncil.org/fibo/ontology/FND/DatesAndTimes/Occurrences/"/>
		<owl:imports rdf:resource="https://spec.edmcouncil.org/fibo/ontology/FND/Organizations/FormalOrganizations/"/>
		<owl:imports rdf:resource="https://spec.edmcouncil.org/fibo/ontology/FND/Utilities/AnnotationVocabulary/"/>
		<owl:versionIRI rdf:resource="https://spec.edmcouncil.org/fibo/ontology/FBC/DebtAndEquities/CreditEvents/"/>
		<fibo-fnd-utl-av:hasMaturityLevel rdf:resource="&fibo-fnd-utl-av;Provisional"/>
	</owl:Ontology>
	
	<owl:Class rdf:about="&fibo-fbc-dae-cre;Bankruptcy">
		<rdfs:subClassOf rdf:resource="&fibo-fbc-dae-cre;CreditEvent"/>
		<rdfs:label xml:lang="en">bankruptcy</rdfs:label>
		<skos:definition xml:lang="en">credit event involving a change in state or condition in which a party becomes insolvent or unable to meet debt obligations</skos:definition>
		<fibo-fnd-utl-av:adaptedFrom>Barron&apos;s Dictionary of Banking Terms, Sixth Edition, 2012</fibo-fnd-utl-av:adaptedFrom>
		<fibo-fnd-utl-av:adaptedFrom rdf:datatype="&xsd;anyURI">https://thelawdictionary.org/bankruptcy/</fibo-fnd-utl-av:adaptedFrom>
	</owl:Class>
	
	<owl:Class rdf:about="&fibo-fbc-dae-cre;BreachOfCovenant">
		<rdfs:subClassOf rdf:resource="&fibo-fbc-dae-cre;CreditEvent"/>
		<rdfs:label xml:lang="en">breach of covenant</rdfs:label>
		<skos:definition xml:lang="en">credit event representing a violation of an express, or implied, condition of a contract to do or not to do something that has a negative financial impact</skos:definition>
	</owl:Class>
	
	<owl:Class rdf:about="&fibo-fbc-dae-cre;CreditEvent">
		<rdfs:subClassOf rdf:resource="&fibo-fnd-dt-oc;Occurrence"/>
		<rdfs:label xml:lang="en">credit event</rdfs:label>
		<skos:definition xml:lang="en">event signifying a sudden change in a borrower&apos;s credit standing, such as bankruptcy or a violation of a bond indenture or loan agreement, that raises doubts about the borrower&apos;s ability to meet current or future obligations</skos:definition>
	</owl:Class>
	
	<owl:Class rdf:about="&fibo-fbc-dae-cre;DefaultEvent">
		<rdfs:subClassOf rdf:resource="&fibo-fbc-dae-cre;CreditEvent"/>
		<rdfs:label xml:lang="en">default event</rdfs:label>
		<skos:definition xml:lang="en">credit event representing a failure to meet a contractual obligation, such as, but not limited to, failure to repay a debt including interest or principal on a loan or security</skos:definition>
		<fibo-fnd-utl-av:explanatoryNote xml:lang="en">A default can occur when a borrower is unable to make timely payments, misses payments, or avoids or stops making payments, typically with respect to a single transaction. A default has adverse effects on the borrower&apos;s credit and ability to borrow in the future.</fibo-fnd-utl-av:explanatoryNote>
	</owl:Class>
	
	<owl:Class rdf:about="&fibo-fbc-dae-cre;DistressedRatingsDowngrade">
		<rdfs:subClassOf rdf:resource="&fibo-fbc-dae-cre;Downgrade"/>
		<rdfs:label xml:lang="en">distressed ratings downgrade</rdfs:label>
		<skos:definition xml:lang="en">credit event triggered when the credit rating of the reference obligation is downgraded to a distressed rating level or the rating is withdrawn by one or more ratings agency</skos:definition>
	</owl:Class>
	
	<owl:Class rdf:about="&fibo-fbc-dae-cre;Downgrade">
		<rdfs:subClassOf rdf:resource="&fibo-fbc-dae-cre;ObligationSpecificCreditEvent"/>
		<rdfs:label xml:lang="en">downgrade</rdfs:label>
		<skos:definition xml:lang="en">credit event triggered when the credit rating of the reference obligation is downgraded</skos:definition>
	</owl:Class>
	
	<owl:Class rdf:about="&fibo-fbc-dae-cre;EntitySpecificCreditEvent">
		<rdfs:subClassOf rdf:resource="&fibo-fbc-dae-cre;CreditEvent"/>
		<rdfs:subClassOf>
			<owl:Restriction>
				<owl:onProperty rdf:resource="&fibo-fnd-rel-rel;involves"/>
				<owl:someValuesFrom rdf:resource="&fibo-fnd-org-fm;FormalOrganization"/>
			</owl:Restriction>
		</rdfs:subClassOf>
		<rdfs:label xml:lang="en">entity-specific credit event</rdfs:label>
		<owl:disjointWith rdf:resource="&fibo-fbc-dae-cre;ObligationSpecificCreditEvent"/>
		<skos:definition xml:lang="en">credit event specified for a given formal organization rather than on a specific reference obligation</skos:definition>
	</owl:Class>
	
	<owl:Class rdf:about="&fibo-fbc-dae-cre;FailureToPay">
		<rdfs:subClassOf rdf:resource="&fibo-fbc-dae-cre;DefaultEvent"/>
		<rdfs:subClassOf>
			<owl:Restriction>
				<owl:onProperty rdf:resource="&fibo-fbc-dae-cre;hasGracePeriod"/>
				<owl:onClass rdf:resource="&fibo-fnd-dt-fd;DatePeriod"/>
				<owl:maxQualifiedCardinality rdf:datatype="&xsd;nonNegativeInteger">1</owl:maxQualifiedCardinality>
			</owl:Restriction>
		</rdfs:subClassOf>
		<rdfs:label xml:lang="en">failure to pay</rdfs:label>
		<skos:definition xml:lang="en">default event that is triggered following any applicable grace period in which a payment obligation is missed</skos:definition>
	</owl:Class>
	
	<owl:Class rdf:about="&fibo-fbc-dae-cre;FailureToPayInterest">
		<rdfs:subClassOf rdf:resource="&fibo-fbc-dae-cre;FailureToPay"/>
		<rdfs:label xml:lang="en">failure to pay interest</rdfs:label>
		<skos:definition xml:lang="en">default event that where either an expected interest payment is missed altogether or the amount paid is less than the required amount</skos:definition>
	</owl:Class>
	
	<owl:Class rdf:about="&fibo-fbc-dae-cre;FailureToPayPrincipal">
		<rdfs:subClassOf rdf:resource="&fibo-fbc-dae-cre;FailureToPay"/>
		<rdfs:label xml:lang="en">failure to pay principal</rdfs:label>
		<skos:definition xml:lang="en">default event that where either an expected principal payment is missed altogether or the amount paid is less than the required amount</skos:definition>
	</owl:Class>
	
	<owl:Class rdf:about="&fibo-fbc-dae-cre;FilingForBankruptcy">
		<rdfs:subClassOf rdf:resource="&fibo-fbc-dae-cre;CreditEvent"/>
		<rdfs:label xml:lang="en">filing for bankruptcy</rdfs:label>
		<skos:definition xml:lang="en">credit event that involves an initial request of a court to be recognized as bankrupt</skos:definition>
		<fibo-fnd-utl-av:explanatoryNote xml:lang="en">The bankruptcy process is initiated via a petition filed by the debtor or on behalf of creditors. The debtor&apos;s assets may be used to repay a portion of outstanding debt as specified by the court or a court-appointed individual.</fibo-fnd-utl-av:explanatoryNote>
	</owl:Class>
	
	<owl:Class rdf:about="&fibo-fbc-dae-cre;HardCreditEvent">
		<rdfs:subClassOf rdf:resource="&fibo-fbc-dae-cre;DefaultEvent"/>
		<rdfs:label xml:lang="en">hard credit event</rdfs:label>
		<skos:definition xml:lang="en">default event that is not repairable</skos:definition>
	</owl:Class>
	
	<owl:Class rdf:about="&fibo-fbc-dae-cre;InstallmentDefault">
		<rdfs:subClassOf rdf:resource="&fibo-fbc-dae-cre;DefaultEvent"/>
		<rdfs:label xml:lang="en">installment default</rdfs:label>
		<skos:definition xml:lang="en">default event involving non-payment of several installment payments as scheduled in the terms of the agreement, or non-payment of a call by the beneficial owner</skos:definition>
		<fibo-fnd-utl-av:explanatoryNote xml:lang="en">The latter may result in a court action by the issuer or the sale of the securities to recover costs and/or a forfeit of partially paid securities.</fibo-fnd-utl-av:explanatoryNote>
	</owl:Class>
	
	<owl:Class rdf:about="&fibo-fbc-dae-cre;MaturityExtension">
		<rdfs:subClassOf rdf:resource="&fibo-fbc-dae-cre;ObligationSpecificCreditEvent"/>
		<rdfs:label xml:lang="en">maturity extension</rdfs:label>
		<skos:definition xml:lang="en">credit event involving extension of payments beyond the original maturity date of the obligation</skos:definition>
		<fibo-fnd-utl-av:explanatoryNote xml:lang="en">As stipulated in the terms and conditions for a bond, for example, the issuer or the bondholder may prolong the maturity date. After extension, the security may differ from original issue (new rate or maturity date). May be subject to bondholder&apos;s approval.</fibo-fnd-utl-av:explanatoryNote>
	</owl:Class>
	
	<owl:Class rdf:about="&fibo-fbc-dae-cre;Moratorium">
		<rdfs:subClassOf rdf:resource="&fibo-fbc-dae-cre;EntitySpecificCreditEvent"/>
		<rdfs:label xml:lang="en">moratorium</rdfs:label>
		<skos:definition xml:lang="en">entity-specific credit event involving a temporary suspension of payments until related issues are resolved</skos:definition>
		<fibo-fnd-utl-av:explanatoryNote xml:lang="en">A moratorium may be a legally-mandated hiatus in debt collection as a part of a bankruptcy process.</fibo-fnd-utl-av:explanatoryNote>
	</owl:Class>
	
	<owl:Class rdf:about="&fibo-fbc-dae-cre;ObligationAcceleration">
		<rdfs:subClassOf rdf:resource="&fibo-fbc-dae-cre;ObligationSpecificCreditEvent"/>
		<rdfs:label xml:lang="en">obligation acceleration</rdfs:label>
		<skos:definition xml:lang="en">credit event triggered when one or more reference obligations become immediately due and payable as a result of a default or covenant breach on the reference entity&apos;s other debt instruments, subject to a materiality threshold</skos:definition>
	</owl:Class>
	
	<owl:Class rdf:about="&fibo-fbc-dae-cre;ObligationDefault">
		<rdfs:subClassOf rdf:resource="&fibo-fbc-dae-cre;DefaultEvent"/>
		<rdfs:subClassOf rdf:resource="&fibo-fbc-dae-cre;ObligationSpecificCreditEvent"/>
		<rdfs:label xml:lang="en">obligation default</rdfs:label>
		<skos:definition xml:lang="en">credit event triggered as a result of an obligation-specific default</skos:definition>
	</owl:Class>
	
	<owl:Class rdf:about="&fibo-fbc-dae-cre;ObligationRestructuring">
		<rdfs:subClassOf rdf:resource="&fibo-fbc-dae-cre;ObligationSpecificCreditEvent"/>
		<rdfs:label xml:lang="en">obligation restructuring</rdfs:label>
		<skos:definition xml:lang="en">entity-specific credit event that materially impacts an obligation, such as an interest rate reduction, principal reduction, deferral of interest or principal, change in priority ranking, or change in currency or composition of payment</skos:definition>
	</owl:Class>
	
	<owl:Class rdf:about="&fibo-fbc-dae-cre;ObligationSpecificCreditEvent">
		<rdfs:subClassOf rdf:resource="&fibo-fbc-dae-cre;CreditEvent"/>
		<rdfs:subClassOf>
			<owl:Restriction>
				<owl:onProperty rdf:resource="&fibo-fnd-rel-rel;involves"/>
				<owl:someValuesFrom rdf:resource="&fibo-fbc-dae-dbt;CreditAgreement"/>
			</owl:Restriction>
		</rdfs:subClassOf>
		<rdfs:label xml:lang="en">obligation-specific credit event</rdfs:label>
		<skos:definition xml:lang="en">credit event that relates to an individual credit agreement or debt instrument (reference obligation)</skos:definition>
	</owl:Class>
	
	<owl:Class rdf:about="&fibo-fbc-dae-cre;Repudiation">
		<rdfs:subClassOf rdf:resource="&fibo-fbc-dae-cre;EntitySpecificCreditEvent"/>
		<rdfs:label xml:lang="en">repudiation</rdfs:label>
		<skos:definition xml:lang="en">entity-specific credit event involving the dispute of the validity of a contract and refusal to honor its terms</skos:definition>
	</owl:Class>
	
	<owl:Class rdf:about="&fibo-fbc-dae-cre;SoftCreditEvent">
		<rdfs:subClassOf rdf:resource="&fibo-fbc-dae-cre;DefaultEvent"/>
		<rdfs:label xml:lang="en">soft credit event</rdfs:label>
		<owl:disjointWith rdf:resource="&fibo-fbc-dae-cre;HardCreditEvent"/>
		<skos:definition xml:lang="en">default event that is repairable</skos:definition>
		<fibo-fnd-utl-av:explanatoryNote xml:lang="en">If the default is not repaired within a grace period, then a failure to repair (failure to pay) credit event is triggered, potentially as a hard default.</fibo-fnd-utl-av:explanatoryNote>
	</owl:Class>
	
	<owl:Class rdf:about="&fibo-fbc-dae-cre;WriteDown">
		<rdfs:subClassOf rdf:resource="&fibo-fbc-dae-cre;ObligationSpecificCreditEvent"/>
		<rdfs:label xml:lang="en">write-down</rdfs:label>
		<skos:definition xml:lang="en">obligation-specific credit event whereby the book value of the obligation, such as the outstanding principal amount, is reduced</skos:definition>
	</owl:Class>
	
	<owl:ObjectProperty rdf:about="&fibo-fbc-dae-cre;hasDefaultThresholdAmount">
		<rdfs:label xml:lang="en">has default threshold amount</rdfs:label>
		<rdfs:domain rdf:resource="&fibo-fbc-dae-cre;EntitySpecificCreditEvent"/>
		<rdfs:range rdf:resource="&fibo-fnd-acc-cur;MonetaryAmount"/>
		<skos:definition xml:lang="en">specifies an amount of money that triggers a repudiation/moratorium or restructuring event</skos:definition>
	</owl:ObjectProperty>
	
	<owl:DatatypeProperty rdf:about="&fibo-fbc-dae-cre;hasExtendableGracePeriod">
		<rdfs:label xml:lang="en">has extendable grace period</rdfs:label>
		<rdfs:domain rdf:resource="&fibo-fbc-dae-cre;FailureToPay"/>
		<rdfs:range rdf:resource="&xsd;boolean"/>
		<skos:definition xml:lang="en">indicates whether or not the grace period may be extended, which may be jurisdiction specific</skos:definition>
	</owl:DatatypeProperty>
	
	<owl:ObjectProperty rdf:about="&fibo-fbc-dae-cre;hasGracePeriod">
		<rdfs:label xml:lang="en">has grace period</rdfs:label>
		<rdfs:domain rdf:resource="&fibo-fbc-dae-cre;FailureToPay"/>
		<rdfs:range rdf:resource="&fibo-fnd-dt-fd;DatePeriod"/>
		<skos:definition xml:lang="en">window following any payment due date during which a party must fulfil its obligations before a failure to pay credit event occurs. Further notes: ISDA 2003 Term: Grace Period. Note this may be a period denominated in business days or calendar days - this is a qualifying fact about the referenced term &quot;Date Period&quot;. FpML full definition: &apos;The number of calendar or business days after any due date that the reference entity has to fulfil its obligations before a failure to pay credit event is deemed to have occurred. ISDA 2003 Term: Grace Period.&apos;</skos:definition>
		<fibo-fnd-utl-av:explanatoryNote xml:lang="en">Note that this may be a period denominated in business days or calendar days.</fibo-fnd-utl-av:explanatoryNote>
	</owl:ObjectProperty>
	
	<owl:ObjectProperty rdf:about="&fibo-fbc-dae-cre;hasPaymentThreshold">
		<rdfs:label xml:lang="en">has payment threshold</rdfs:label>
		<rdfs:domain rdf:resource="&fibo-fbc-dae-cre;FailureToPay"/>
		<rdfs:range rdf:resource="&fibo-fnd-acc-cur;MonetaryAmount"/>
		<skos:definition xml:lang="en">indicates a threshold with respect to triggering the failure to pay event</skos:definition>
		<fibo-fnd-utl-av:explanatoryNote xml:lang="en">Market standard is USD 1,000,000 (JPY 100,000,000 for Japanese Yen trades) or its equivalent in the relevant obligation currency. This is applied on an aggregate basis across all Obligations of the Reference Entity. Intended to prevent technical/operational errors from triggering credit events.</fibo-fnd-utl-av:explanatoryNote>
	</owl:ObjectProperty>
	
	<owl:DatatypeProperty rdf:about="&fibo-fbc-dae-cre;involvesMultipleEvents">
		<rdfs:label xml:lang="en">involves multiple events</rdfs:label>
		<rdfs:domain rdf:resource="&fibo-fbc-dae-cre;ObligationRestructuring"/>
		<rdfs:range rdf:resource="&xsd;boolean"/>
		<skos:definition xml:lang="en">indicates that the restructuring actually involves more than one credit event</skos:definition>
	</owl:DatatypeProperty>
	
	<owl:DatatypeProperty rdf:about="&fibo-fbc-dae-cre;involvesMultipleHolders">
		<rdfs:label xml:lang="en">multiple holder obligation</rdfs:label>
		<rdfs:domain rdf:resource="&fibo-fbc-dae-cre;ObligationRestructuring"/>
		<rdfs:range rdf:resource="&xsd;boolean"/>
		<skos:definition xml:lang="en">indicates that the obligation is held by more than three holders that are not affiliates of each other and where at least two thirds of the holders must agree to the event that constitutes the restructuring credit event</skos:definition>
	</owl:DatatypeProperty>

</rdf:RDF>