<?xml version="1.0" encoding="UTF-8"?>
<!DOCTYPE rdf:RDF [
	<!ENTITY dct "http://purl.org/dc/terms/">
	<!ENTITY fibo-be-fct-fct "https://spec.edmcouncil.org/fibo/BE/FunctionalEntities/FunctionalEntities/">
	<!ENTITY fibo-be-fct-pub "https://spec.edmcouncil.org/fibo/BE/FunctionalEntities/Publishers/">
	<!ENTITY fibo-fnd-arr-doc "https://spec.edmcouncil.org/fibo/FND/Arrangements/Documents/">
	<!ENTITY fibo-fnd-org-fm "https://spec.edmcouncil.org/fibo/FND/Organizations/FormalOrganizations/">
	<!ENTITY fibo-fnd-pty-pty "https://spec.edmcouncil.org/fibo/FND/Parties/Parties/">
	<!ENTITY fibo-fnd-pty-rl "https://spec.edmcouncil.org/fibo/FND/Parties/Roles/">
	<!ENTITY fibo-fnd-rel-rel "https://spec.edmcouncil.org/fibo/FND/Relations/Relations/">
	<!ENTITY fibo-fnd-utl-av "https://spec.edmcouncil.org/fibo/FND/Utilities/AnnotationVocabulary/">
	<!ENTITY owl "http://www.w3.org/2002/07/owl#">
	<!ENTITY rdf "http://www.w3.org/1999/02/22-rdf-syntax-ns#">
	<!ENTITY rdfs "http://www.w3.org/2000/01/rdf-schema#">
	<!ENTITY skos "http://www.w3.org/2004/02/skos/core#">
	<!ENTITY sm "http://www.omg.org/techprocess/ab/SpecificationMetadata/">
	<!ENTITY xsd "http://www.w3.org/2001/XMLSchema#">
]>
<rdf:RDF
	xml:base="https://spec.edmcouncil.org/fibo/BE/FunctionalEntities/Publishers/"
	xmlns:dct="http://purl.org/dc/terms/"
	xmlns:fibo-be-fct-fct="https://spec.edmcouncil.org/fibo/BE/FunctionalEntities/FunctionalEntities/"
	xmlns:fibo-be-fct-pub="https://spec.edmcouncil.org/fibo/BE/FunctionalEntities/Publishers/"
	xmlns:fibo-fnd-arr-doc="https://spec.edmcouncil.org/fibo/FND/Arrangements/Documents/"
	xmlns:fibo-fnd-org-fm="https://spec.edmcouncil.org/fibo/FND/Organizations/FormalOrganizations/"
	xmlns:fibo-fnd-pty-pty="https://spec.edmcouncil.org/fibo/FND/Parties/Parties/"
	xmlns:fibo-fnd-pty-rl="https://spec.edmcouncil.org/fibo/FND/Parties/Roles/"
	xmlns:fibo-fnd-rel-rel="https://spec.edmcouncil.org/fibo/FND/Relations/Relations/"
	xmlns:fibo-fnd-utl-av="https://spec.edmcouncil.org/fibo/FND/Utilities/AnnotationVocabulary/"
	xmlns:owl="http://www.w3.org/2002/07/owl#"
	xmlns:rdf="http://www.w3.org/1999/02/22-rdf-syntax-ns#"
	xmlns:rdfs="http://www.w3.org/2000/01/rdf-schema#"
	xmlns:skos="http://www.w3.org/2004/02/skos/core#"
	xmlns:sm="http://www.omg.org/techprocess/ab/SpecificationMetadata/"
	xmlns:xsd="http://www.w3.org/2001/XMLSchema#">
	
	<owl:Ontology
		rdf:about="https://spec.edmcouncil.org/fibo/BE/FunctionalEntities/Publishers/">
		<rdfs:label>Publishers Ontology</rdfs:label>
		<dct:license
			rdf:datatype="&xsd;anyURI">http://www.omg.org/techprocess/ab/SpecificationMetadata/MITLicense</dct:license>
		<sm:contentLanguage
			rdf:datatype="&xsd;anyURI">http://www.omg.org/spec/ODM/</sm:contentLanguage>
		<sm:contentLanguage
			rdf:datatype="&xsd;anyURI">http://www.w3.org/standards/techs/owl#w3c_all</sm:contentLanguage>
		<sm:copyright>Copyright (c) 2013-2016 EDM Council, Inc.
Copyright (c) 2013-2016 Object Management Group, Inc.</sm:copyright>
		<sm:dependsOn
			rdf:datatype="&xsd;anyURI">https://spec.edmcouncil.org/fibo/BE/FunctionalEntities/FunctionalEntities/</sm:dependsOn>
		<sm:dependsOn
			rdf:datatype="&xsd;anyURI">https://spec.edmcouncil.org/fibo/FND/</sm:dependsOn>
		<sm:fileAbbreviation>fibo-be-fct-pub</sm:fileAbbreviation>
		<sm:fileAbstract>This ontology defines the fundamental concepts for publishers of information, including entities whose primary function is to publish, and entities (whether or not they are publishers in that sense) which are in the role of the publisher of some information. This ontology also includes the published information itself, i.e. the publication.</sm:fileAbstract>
		<sm:filename>Publishers.rdf</sm:filename>
		<rdfs:seeAlso
			rdf:datatype="&xsd;anyURI">https://spec.edmcouncil.org/fibo/AboutTheEDMC-FIBOFamily/</rdfs:seeAlso>
		<rdfs:seeAlso
			rdf:datatype="&xsd;anyURI">https://spec.edmcouncil.org/fibo/BE/AboutBE/</rdfs:seeAlso>
		<rdfs:seeAlso
			rdf:datatype="&xsd;anyURI">https://spec.edmcouncil.org/fibo/BE/FunctionalEntities/AboutFunctionalEntities/</rdfs:seeAlso>
		<owl:imports
			rdf:resource="https://spec.edmcouncil.org/fibo/BE/FunctionalEntities/FunctionalEntities/"/>
		<owl:imports
			rdf:resource="https://spec.edmcouncil.org/fibo/FND/Arrangements/Documents/"/>
		<owl:imports
			rdf:resource="https://spec.edmcouncil.org/fibo/FND/Organizations/FormalOrganizations/"/>
		<owl:imports
			rdf:resource="https://spec.edmcouncil.org/fibo/FND/Parties/Parties/"/>
		<owl:imports
			rdf:resource="https://spec.edmcouncil.org/fibo/FND/Parties/Roles/"/>
		<owl:imports
			rdf:resource="https://spec.edmcouncil.org/fibo/FND/Relations/Relations/"/>
		<owl:imports
			rdf:resource="https://spec.edmcouncil.org/fibo/FND/Utilities/AnnotationVocabulary/"/>
		<owl:versionIRI
			rdf:resource="https://spec.edmcouncil.org/fibo/BE/20160201/FunctionalEntities/Publishers/"/>
		<skos:changeNote>The https://spec.edmcouncil.org/fibo/BE/20140501/FunctionalEntities/Publishers.rdf version of this ontology was modified per the issue resolutions identified in the FIBO BE 1.0 FTF report.</skos:changeNote>
	</owl:Ontology>
	
	<owl:Class
		rdf:about="&fibo-be-fct-pub;Publication">
		<rdfs:subClassOf
			rdf:resource="&fibo-fnd-arr-doc;Document"/>
		<rdfs:label>publication</rdfs:label>
		<skos:definition>anything made public by print (such as a newspaper, magazine, pamphlet, letter, telegram, via computer modem or program, or in a poster, brochure or pamphlet), orally, or by broadcast (radio, television)</skos:definition>
		<fibo-fnd-utl-av:adaptedFrom
			rdf:datatype="&xsd;anyURI">http://legal-dictionary.thefreedictionary.com/Publication</fibo-fnd-utl-av:adaptedFrom>
	</owl:Class>
	
	<owl:Class
		rdf:about="&fibo-be-fct-pub;Publisher">
		<rdfs:subClassOf
			rdf:resource="&fibo-fnd-pty-pty;PartyInRole"/>
		<rdfs:subClassOf>
			<owl:Restriction>
				<owl:onClass
					rdf:resource="&fibo-fnd-pty-pty;IndependentParty"/>
				<owl:onProperty
					rdf:resource="&fibo-fnd-rel-rel;hasIdentity"/>
				<owl:qualifiedCardinality
					rdf:datatype="&xsd;nonNegativeInteger">1</owl:qualifiedCardinality>
			</owl:Restriction>
		</rdfs:subClassOf>
		<rdfs:label>publisher</rdfs:label>
		<skos:definition>a party responsible for the printing or distribution of digital or printed information</skos:definition>
		<fibo-fnd-utl-av:adaptedFrom
			rdf:datatype="&xsd;anyURI">http://www.businessdictionary.com/definition/publisher.html</fibo-fnd-utl-av:adaptedFrom>
		<fibo-fnd-utl-av:explanatoryNote>Typically this role is filled by some entity whose function is that of a publishing house (sometimes also referred to as a publisher, in that different sense). Publishers may also include banks, government agencies and the like.</fibo-fnd-utl-av:explanatoryNote>
	</owl:Class>
	
	<owl:Class
		rdf:about="&fibo-be-fct-pub;PublishingHouse">
		<rdfs:subClassOf
			rdf:resource="&fibo-be-fct-fct;FunctionalBusinessEntity"/>
		<rdfs:subClassOf>
			<owl:Restriction>
				<owl:onClass
					rdf:resource="&fibo-fnd-org-fm;FormalOrganization"/>
				<owl:onProperty
					rdf:resource="&fibo-fnd-rel-rel;hasIdentity"/>
				<owl:qualifiedCardinality
					rdf:datatype="&xsd;nonNegativeInteger">1</owl:qualifiedCardinality>
			</owl:Restriction>
		</rdfs:subClassOf>
		<rdfs:label>publishing house</rdfs:label>
		<skos:definition>some organization whose principal role is to publish information</skos:definition>
		<skos:scopeNote>Publishing house in the sense intended here includes any organization whose role is to make information publicly available whether by disemminating it directly or indirectly and regardless of the type of information. These include organizations whose primary function is that of a market data vendor.</skos:scopeNote>
	</owl:Class>
	
	<owl:ObjectProperty
		rdf:about="&fibo-be-fct-pub;hasPublisher">
		<rdfs:label>has publisher</rdfs:label>
		<rdfs:domain
			rdf:resource="&fibo-be-fct-pub;Publication"/>
		<rdfs:range
			rdf:resource="&fibo-be-fct-pub;Publisher"/>
		<owl:inverseOf
			rdf:resource="&fibo-be-fct-pub;publishes"/>
		<skos:definition>some person or organization whose role it has been to publish this information</skos:definition>
	</owl:ObjectProperty>
	
	<owl:ObjectProperty
		rdf:about="&fibo-be-fct-pub;isPublishedBy">
		<rdfs:label>is published by</rdfs:label>
		<rdfs:domain
			rdf:resource="&fibo-be-fct-pub;Publication"/>
		<rdfs:range
			rdf:resource="&fibo-fnd-pty-pty;IndependentParty"/>
		<skos:definition>identifies the independent party (i.e., the individual or organization) that disseminates the material</skos:definition>
	</owl:ObjectProperty>
	
	<owl:ObjectProperty
		rdf:about="&fibo-be-fct-pub;publishes">
		<rdfs:label>publishes</rdfs:label>
		<rdfs:domain
			rdf:resource="&fibo-be-fct-pub;Publisher"/>
		<rdfs:range
			rdf:resource="&fibo-be-fct-pub;Publication"/>
		<skos:definition>prepares and issues material for public consumption</skos:definition>
		<fibo-fnd-utl-av:definitionOrigin
			rdf:datatype="&xsd;anyURI">http://www.thefreedictionary.com/publish</fibo-fnd-utl-av:definitionOrigin>
	</owl:ObjectProperty>

</rdf:RDF>