<?xml version="1.0" encoding="UTF-8"?>
<rdf:RDF xmlns:xsd="http://www.w3.org/2001/XMLSchema#"
         xmlns:sm="http://www.omg.org/techprocess/ab/SpecificationMetadata/"
         xmlns:fibo-fnd-utl-av="http://www.omg.org/spec/EDMC-FIBO/FND/Utilities/AnnotationVocabulary/"
         xmlns:rdf="http://www.w3.org/1999/02/22-rdf-syntax-ns#"
         xmlns:rdfs="http://www.w3.org/2000/01/rdf-schema#"
         xmlns:owl="http://www.w3.org/2002/07/owl#"
         xmlns:skos="http://www.w3.org/2004/02/skos/core#"
         xmlns:dc="http://purl.org/dc/terms/"
         xml:base="http://www.edmcouncil.org/spec/EDMC-SR/FND/LawExt/JurisdictionExtended/">

   <owl:Ontology rdf:about="http://www.edmcouncil.org/spec/EDMC-SR/FND/LawExt/JurisdictionExtended/">
      <owl:imports rdf:resource="http://www.omg.org/spec/EDMC-SR/FND/Law/Jurisdictions/"/>
   </owl:Ontology>

   <!--Datatypes-->

<!--Object Properties-->

<owl:ObjectProperty rdf:about="http://www.edmcouncil.org/spec/EDMC-SR/FND/LawExt/JurisdictionExtended/bijuridicialJurisdictionPartiallyGovernedUnderCivilLawSystem">
      <skos:definition>One system of law under which a Bijuridicial Jurisdiction is governed is the system of Civil Law.</skos:definition>
      <skos:editorialNote>A Bijuridicial Jurisdiction is governed under two systems of law, of which this is one.</skos:editorialNote>
      <rdfs:subPropertyOf rdf:resource="http://www.omg.org/spec/EDMC-SR/FND/Law/Jurisdictions/jurisdictionGovernedBy"/>
      <rdfs:domain rdf:resource="http://www.edmcouncil.org/spec/EDMC-SR/FND/LawExt/JurisdictionExtended/BijuridicialJurisdiction"/>
      <rdfs:range rdf:resource="http://www.omg.org/spec/EDMC-SR/FND/Law/Jurisdictions/CivilLawSystem"/>
   </owl:ObjectProperty>

   <owl:ObjectProperty rdf:about="http://www.edmcouncil.org/spec/EDMC-SR/FND/LawExt/JurisdictionExtended/bijuridicialJurisdictionPartiallyGovernedUnderCommonLawSystem">
      <skos:definition>One system of law under which a Bijuridicial Jurisdiction is governed is the system of Common Law.</skos:definition>
      <skos:editorialNote>A Bijuridicial Jurisdiction is governed under two systems of law, of which this is one.</skos:editorialNote>
      <rdfs:subPropertyOf rdf:resource="http://www.omg.org/spec/EDMC-SR/FND/Law/Jurisdictions/jurisdictionGovernedBy"/>
      <rdfs:domain rdf:resource="http://www.edmcouncil.org/spec/EDMC-SR/FND/LawExt/JurisdictionExtended/BijuridicialJurisdiction"/>
      <rdfs:range rdf:resource="http://www.omg.org/spec/EDMC-SR/FND/Law/Jurisdictions/CommonLawSystem"/>
   </owl:ObjectProperty>

   <owl:ObjectProperty rdf:about="http://www.edmcouncil.org/spec/EDMC-SR/FND/LawExt/JurisdictionExtended/incorporatesSome">
      <skos:definition>The laws included in this Body of Law.</skos:definition>
      <rdfs:domain rdf:resource="http://www.edmcouncil.org/spec/EDMC-SR/FND/LawExt/JurisdictionExtended/BodyOfLaw"/>
      <rdfs:range rdf:resource="http://www.omg.org/spec/EDMC-SR/FND/Law/LegalCore/Law"/>
   </owl:ObjectProperty>

   <owl:ObjectProperty rdf:about="http://www.edmcouncil.org/spec/EDMC-SR/FND/LawExt/JurisdictionExtended/hasInForce">
      <rdfs:domain rdf:resource="http://www.omg.org/spec/EDMC-SR/FND/Law/Jurisdictions/Jurisdiction"/>
      <rdfs:range rdf:resource="http://www.omg.org/spec/EDMC-SR/FND/Law/Jurisdictions/StatuteLaw"/>
      <owl:inverseOf rdf:resource="http://www.omg.org/spec/EDMC-SR/FND/Law/Jurisdictions/isInForceIn"/>
   </owl:ObjectProperty>

   <owl:ObjectProperty rdf:about="http://www.edmcouncil.org/spec/EDMC-SR/FND/LawExt/JurisdictionExtended/definesTheApplicationOf">
      <skos:definition>The Body of Law, the application of which is defined in the Legal System.</skos:definition>
      <rdfs:domain rdf:resource="http://www.omg.org/spec/EDMC-SR/FND/Law/Jurisdictions/LegalSystem"/>
      <rdfs:range rdf:resource="http://www.edmcouncil.org/spec/EDMC-SR/FND/LawExt/JurisdictionExtended/BodyOfLaw"/>
   </owl:ObjectProperty>

   <owl:ObjectProperty rdf:about="http://www.edmcouncil.org/spec/EDMC-SR/FND/LawExt/JurisdictionExtended/religiousLawJurisdictionGovernedUnder">
      <skos:definition>The system of law under which a Religious Law Jurisdiction is governed. This is some system of Religious Law.</skos:definition>
      <skos:editorialNote>There are several mutually incompatible systems of Religious Law - the term referred to here is ancestral to all of those and defines simply that the jurisdiction in question is some kind of religious law jurisdiction - specific types are to be defined per system of religious law (two are included in the model for reference and possible use; there may be others).</skos:editorialNote>
      <rdfs:subPropertyOf rdf:resource="http://www.omg.org/spec/EDMC-SR/FND/Law/Jurisdictions/jurisdictionGovernedBy"/>
      <rdfs:domain rdf:resource="http://www.edmcouncil.org/spec/EDMC-SR/FND/LawExt/JurisdictionExtended/ReligiousLawJurisdiction"/>
      <rdfs:range rdf:resource="http://www.edmcouncil.org/spec/EDMC-SR/FND/LawExt/JurisdictionExtended/ReligiousLawSystem"/>
   </owl:ObjectProperty>

   <owl:ObjectProperty rdf:about="http://www.edmcouncil.org/spec/EDMC-SR/FND/LawExt/JurisdictionExtended/shariaLawJurisdictionGovernedUnder">
      <skos:definition>The system of law under which a Shari'a Law Jurisdiction is governed. This is the system of Shari'a Law.</skos:definition>
      <rdfs:subPropertyOf rdf:resource="http://www.edmcouncil.org/spec/EDMC-SR/FND/LawExt/JurisdictionExtended/religiousLawJurisdictionGovernedUnder"/>
      <rdfs:domain rdf:resource="http://www.edmcouncil.org/spec/EDMC-SR/FND/LawExt/JurisdictionExtended/ShariaLawJurisdiction"/>
      <rdfs:range rdf:resource="http://www.edmcouncil.org/spec/EDMC-SR/FND/LawExt/JurisdictionExtended/ShariaLawSystem"/>
   </owl:ObjectProperty>

   <owl:ObjectProperty rdf:about="http://www.edmcouncil.org/spec/EDMC-SR/FND/LawExt/JurisdictionExtended/constrainsStatuteLaw">
      <skos:definition>The Constitution constrains what can or cannot be legislated as Law for the Jurisdiction in which that Constitution applies.</skos:definition>
      <rdfs:subPropertyOf rdf:resource="http://www.omg.org/spec/EDMC-SR/FND/Law/LegalCore/governs"/>
      <rdfs:domain rdf:resource="http://www.omg.org/spec/EDMC-SR/FND/Law/LegalCore/GovernmentalConstitution"/>
      <rdfs:range rdf:resource="http://www.omg.org/spec/EDMC-SR/FND/Law/Jurisdictions/StatuteLaw"/>
   </owl:ObjectProperty>

   <owl:ObjectProperty rdf:about="http://www.edmcouncil.org/spec/EDMC-SR/FND/LawExt/JurisdictionExtended/governsLegalSystem">
      <rdfs:domain rdf:resource="http://www.omg.org/spec/EDMC-SR/FND/Law/LegalCore/GovernmentalConstitution"/>
      <rdfs:range rdf:resource="http://www.omg.org/spec/EDMC-SR/FND/Law/Jurisdictions/LegalSystem"/>
      <owl:inverseOf rdf:resource="http://www.omg.org/spec/EDMC-SR/FND/Law/Jurisdictions/legalSystemIsGovernedBy"/>
   </owl:ObjectProperty>

   <!--Data Properties-->

<!--Annotation Properties-->

<!--Classes-->

<owl:Class rdf:about="http://www.edmcouncil.org/spec/EDMC-SR/FND/LawExt/JurisdictionExtended/BijuridicialJurisdiction">
      <rdfs:label>Bijuridicial Jurisdiction</rdfs:label>
      <skos:definition>A Jurisdiction in which two or more systems of law are in force.</skos:definition>
      <skos:editorialNote>Examples include South Africa, Quebec, Louisiana and a few others, where or example Civil Law and Common Law arrangements are in force.</skos:editorialNote>
      <rdfs:subClassOf rdf:resource="http://www.omg.org/spec/EDMC-SR/FND/Law/Jurisdictions/Jurisdiction"/>
   </owl:Class>

   <owl:Class rdf:about="http://www.edmcouncil.org/spec/EDMC-SR/FND/LawExt/JurisdictionExtended/BodyOfLaw">
      <rdfs:label>Body Of Law</rdfs:label>
      <skos:definition>Some body of law, that is some set of laws, statutes, ordinances and the like.</skos:definition>
      <rdfs:subClassOf rdf:resource="http://www.edmcouncil.org/spec/EDMC-SR/UO/OntologicalDegree/IndependentThing"/>
   </owl:Class>

   <owl:Class rdf:about="http://www.edmcouncil.org/spec/EDMC-SR/FND/LawExt/JurisdictionExtended/CanonLawSystem">
      <rdfs:label>Canon Law System</rdfs:label>
      <skos:definition>The body of laws &amp; regulations made or adopted by ecclesiastical authority, for the government of the Christian organization and its members.</skos:definition>
      <skos:editorialNote>In force in both the Western (Roman) and Eastern churches, and in some form in the Anglican Church. There appear to be no current instances national jurisdictions which take this as a legal framework, with the possible exception of the Vatican. In historical contexts there would be.</skos:editorialNote>
      <rdfs:subClassOf rdf:resource="http://www.edmcouncil.org/spec/EDMC-SR/FND/LawExt/JurisdictionExtended/ReligiousLawSystem"/>
   </owl:Class>

   <owl:Class rdf:about="http://www.edmcouncil.org/spec/EDMC-SR/FND/LawExt/JurisdictionExtended/CivilLaw">
      <rdfs:label>Civil Law</rdfs:label>
      <skos:definition>The branch of the law dealing with disputes between individuals or organizations, in which compensation may be awarded to the victim.</skos:definition>
      <rdfs:subClassOf rdf:resource="http://www.edmcouncil.org/spec/EDMC-SR/FND/LawExt/JurisdictionExtended/CommonLaw"/>
   </owl:Class>

   <owl:Class rdf:about="http://www.edmcouncil.org/spec/EDMC-SR/FND/LawExt/JurisdictionExtended/CommonLaw">
      <rdfs:label>Common law</rdfs:label>
      <skos:definition>Law developed by judges through decisions of courts and similar tribunals rather than through legislative statutes or executive branch action.</skos:definition>
      <rdfs:subClassOf rdf:resource="http://www.edmcouncil.org/spec/EDMC-SR/FND/LawExt/JurisdictionExtended/BodyOfLaw"/>
   </owl:Class>

   <owl:Class rdf:about="http://www.edmcouncil.org/spec/EDMC-SR/FND/LawExt/JurisdictionExtended/ConstitutionalLaw">
      <rdfs:label>Constitutional Law</rdfs:label>
      <skos:definition>The body of law which defines the relationship of different entities within a state, namely the executive, legislature and the judiciary. Further notes: (from Wikipedia): Constitutional laws may be considered second order rulemaking or rules about making rules to exercise power.</skos:definition>
   </owl:Class>

   <owl:Class rdf:about="http://www.edmcouncil.org/spec/EDMC-SR/FND/LawExt/JurisdictionExtended/CriminalLaw">
      <rdfs:label>Criminal Law</rdfs:label>
      <skos:definition>The body of law that defines conduct that is not allowed because it is held to threaten, harm or endanger the safety and welfare of people, and that sets out the punishments to be imposed on people who do not obey these laws.</skos:definition>
   </owl:Class>

   <owl:Class rdf:about="http://www.edmcouncil.org/spec/EDMC-SR/FND/LawExt/JurisdictionExtended/InternationalLaw">
      <rdfs:label>International Law</rdfs:label>
      <skos:definition>The set of rules generally regarded and accepted as binding in relations between states and nations.</skos:definition>
      <skos:editorialNote>This can refer to three distinct legal disciplines: 1. Public international law governing the relations between provinces and national entities 2. Private international lse, which addresses questions of which jurisdiction may hear a case and which jurisdiction applies to issues in a case 3. Supranational law which concerns regional agreements where the laws of nation states may be held inapplicable when conflicting with a supranational legal system.</skos:editorialNote>
   </owl:Class>

   <owl:Class rdf:about="http://www.edmcouncil.org/spec/EDMC-SR/FND/LawExt/JurisdictionExtended/ReligiousLaw">
      <rdfs:label>Religious Law</rdfs:label>
      <skos:definition>Some set of laws derived from and practised in the name of some religion.</skos:definition>
   </owl:Class>

   <owl:Class rdf:about="http://www.edmcouncil.org/spec/EDMC-SR/FND/LawExt/JurisdictionExtended/ReligiousLawJurisdiction">
      <rdfs:label>Religious Law Jurisdiction</rdfs:label>
      <skos:definition>A Jurisdiction in which some system of religious law is in force.</skos:definition>
      <skos:editorialNote>This includes Sharia Law jurisdictions.</skos:editorialNote>
   </owl:Class>

   <owl:Class rdf:about="http://www.edmcouncil.org/spec/EDMC-SR/FND/LawExt/JurisdictionExtended/ReligiousLawSystem">
      <rdfs:label>Religious Law System</rdfs:label>
      <skos:definition>Some system of law based on the ordering principle of reality as being knowledge as revealed by God and governing all human affairs.</skos:definition>
      <rdfs:subClassOf rdf:resource="http://www.omg.org/spec/EDMC-SR/FND/Law/Jurisdictions/LegalSystem"/>
   </owl:Class>

   <owl:Class rdf:about="http://www.edmcouncil.org/spec/EDMC-SR/FND/LawExt/JurisdictionExtended/ShariaLawJurisdiction">
      <rdfs:label>Sharia Law Jurisdiction</rdfs:label>
      <skos:definition>A Jurisdiction in which a Shari'a system of law is in force.</skos:definition>
      <rdfs:subClassOf rdf:resource="http://www.edmcouncil.org/spec/EDMC-SR/FND/LawExt/JurisdictionExtended/ReligiousLawJurisdiction"/>
   </owl:Class>

   <owl:Class rdf:about="http://www.edmcouncil.org/spec/EDMC-SR/FND/LawExt/JurisdictionExtended/ShariaLawSystem">
      <rdfs:label>Sharia Law System</rdfs:label>
      <skos:definition>A system of Shari'a Law.</skos:definition>
      <skos:editorialNote>There are several schools of law in Islamic jurisprudence; these are not articulated here at present. The bodies of law and other textual corpora referred to in the implementation of this system of law are the Qur'an and the Hadith, with variations in interpretation and precedence according to the system (school) in question. Also known as the Qanun 'Islami (Islamic Canon)</skos:editorialNote>
   </owl:Class>

   <owl:Class rdf:about="http://www.edmcouncil.org/spec/EDMC-SR/FND/LawExt/JurisdictionExtended/StatutoryLaw">
      <rdfs:label>Statutory Law</rdfs:label>
      <skos:definition>Written law set down by a legislature or by a legislator.</skos:definition>
      <skos:editorialNote>Statutory Law may originate with national, state legislatures or local municipalities. Statutes of lower jurisdictions are subordinate to the law of higher. Definition adapted from: Wikipedia</skos:editorialNote>
   </owl:Class>

   <!--Individuals-->

</rdf:RDF>