<?xml version="1.0" encoding="UTF-8"?>
  
<!DOCTYPE rdf:RDF [
    <!ENTITY fibo-be-oacx-ber "http://spec.edmcouncil.org/fibo/red/be/ownership-control-ext/be-relations/">
    <!ENTITY fibo-fnd-pty-pty "http://spec.edmcouncil.org/fibo/red/fnd/parties/parties/">
    <!ENTITY fibo-be-corp-corp "http://spec.edmcouncil.org/fibo/red/be/corporations/corporations/">
    <!ENTITY fibo-be-le-fbo "http://spec.edmcouncil.org/fibo/red/be/legal-entities/formal-business-organizations/">
    <!ENTITY fibo-fnd-aap-agt "http://spec.edmcouncil.org/fibo/red/fnd/agents-and-people/agents/">
]>

<rdf:RDF xmlns:xsd="http://www.w3.org/2001/XMLSchema#"
         xmlns:sm="http://www.omg.org/techprocess/ab/SpecificationMetadata/"
         xmlns:xs="http://www.w3.org/2001/XMLSchema"
         xmlns:fibo-fnd-utl-av="http://www.omg.org/spec/EDMC-FIBO/FND/Utilities/AnnotationVocabulary/"
         xmlns:rdf="http://www.w3.org/1999/02/22-rdf-syntax-ns#"
         xmlns:rdfs="http://www.w3.org/2000/01/rdf-schema#"
         xmlns:owl="http://www.w3.org/2002/07/owl#"
         xmlns:skos="http://www.w3.org/2004/02/skos/core#"
         xmlns:dc="http://purl.org/dc/terms/"
         xml:base="http://spec.edmcouncil.org/fibo/red/be/ownership-control-ext/be-relations/">

   <owl:Ontology rdf:about="http://spec.edmcouncil.org/fibo/red/be/ownership-control-ext/be-relations/">
      <owl:imports rdf:resource="http://spec.edmcouncil.org/fibo/red/fnd/parties/parties/"/>
      <owl:imports rdf:resource="http://spec.edmcouncil.org/fibo/red/be/corporations/corporations/"/>
      <owl:imports rdf:resource="http://spec.edmcouncil.org/fibo/red/be/legal-entities/formal-business-organizations/"/>
      <owl:imports rdf:resource="http://spec.edmcouncil.org/fibo/red/fnd/agents-and-people/agents/"/>
   </owl:Ontology>


  <!--
    ///////////////////////////////////////////////////////////////////////////////////////
    //
    // Datatypes
    //
    ///////////////////////////////////////////////////////////////////////////////////////
    -->



  <!--
    ///////////////////////////////////////////////////////////////////////////////////////
    //
    // Object Properties
    //
    ///////////////////////////////////////////////////////////////////////////////////////
    -->


<owl:ObjectProperty rdf:about="&fibo-be-oacx-ber;constitutionallyPartOwnedBy">
      <rdfs:label>constitutionally part owned by</rdfs:label>
      <skos:definition>Some entity which part owns the Formal Organization by means of some formal instrument such as shares or stockholder equity.</skos:definition>
      <rdfs:subPropertyOf rdf:resource="&fibo-be-oacx-ber;partOwnedBy"/>
      <rdfs:domain rdf:resource="&fibo-be-le-fbo;FormallyConstitutedOrganization"/>
      <rdfs:range rdf:resource="&fibo-fnd-pty-pty;IndependentParty"/>
   </owl:ObjectProperty>

   <owl:ObjectProperty rdf:about="&fibo-be-oacx-ber;controlledBy">
      <rdfs:label>controlled by</rdfs:label>
      <skos:definition>Some entity which controls the Formal Organization, this being some kind of autonomous agent.</skos:definition>
      <rdfs:domain rdf:resource="&fibo-be-le-fbo;FormallyConstitutedOrganization"/>
      <rdfs:range rdf:resource="&fibo-fnd-aap-agt;AutonomousAgent"/>
   </owl:ObjectProperty>

   <owl:ObjectProperty rdf:about="&fibo-be-oacx-ber;hasLegalControlOf">
      <rdfs:label>has legal control of</rdfs:label>
      <skos:definition>The entity has legal control over this organization.</skos:definition>
      <rdfs:domain rdf:resource="&fibo-fnd-pty-pty;IndependentParty"/>
      <rdfs:range rdf:resource="&fibo-be-le-fbo;FormallyConstitutedOrganization"/>
   </owl:ObjectProperty>

   <owl:ObjectProperty rdf:about="&fibo-be-oacx-ber;hasShareholder">
      <rdfs:label>has shareholder</rdfs:label>
      <skos:definition>Some entity which part owns the Incorporated Company by means of shares.</skos:definition>
      <rdfs:subPropertyOf rdf:resource="&fibo-be-oacx-ber;constitutionallyPartOwnedBy"/>
      <rdfs:domain rdf:resource="&fibo-be-corp-corp;IncorporatedCompany"/>
      <rdfs:range rdf:resource="&fibo-fnd-pty-pty;IndependentParty"/>
   </owl:ObjectProperty>

   <owl:ObjectProperty rdf:about="&fibo-be-oacx-ber;hasShareholderFormalOrganization">
      <rdfs:label>has shareholder formal organization</rdfs:label>
      <skos:definition>Some Formal Organization which part owns the Incorporated Company by means of shares.</skos:definition>
      <rdfs:subPropertyOf rdf:resource="&fibo-be-oacx-ber;hasShareholder"/>
      <rdfs:domain rdf:resource="&fibo-be-corp-corp;IncorporatedCompany"/>
      <rdfs:range rdf:resource="&fibo-be-le-fbo;FormallyConstitutedOrganization"/>
   </owl:ObjectProperty>

   <owl:ObjectProperty rdf:about="&fibo-be-oacx-ber;legallyControlledBy">
      <rdfs:label>legally controlled by</rdfs:label>
      <rdfs:subPropertyOf rdf:resource="&fibo-be-oacx-ber;controlledBy"/>
      <rdfs:domain rdf:resource="&fibo-be-le-fbo;FormallyConstitutedOrganization"/>
      <rdfs:range rdf:resource="&fibo-fnd-pty-pty;IndependentParty"/>
      <owl:inverseOf rdf:resource="&fibo-be-oacx-ber;hasLegalControlOf"/>
   </owl:ObjectProperty>

   <owl:ObjectProperty rdf:about="&fibo-be-oacx-ber;majorityControllingInterestBy">
      <rdfs:label>majority controlling interest by</rdfs:label>
      <skos:definition>Entity having controlling ownership of the Formal Organization.</skos:definition>
      <rdfs:domain rdf:resource="&fibo-be-le-fbo;FormallyConstitutedOrganization"/>
      <rdfs:range rdf:resource="&fibo-fnd-pty-pty;IndependentParty"/>
   </owl:ObjectProperty>

   <owl:ObjectProperty rdf:about="&fibo-be-oacx-ber;majorityControllingOwnershipBy">
      <rdfs:label>majority controlling ownership by</rdfs:label>
      <skos:definition>Incorporated Company holding over fifty percent of the voting shares in this Incorporated Company.</skos:definition>
      <rdfs:subPropertyOf rdf:resource="&fibo-be-oacx-ber;someControllingInterestByCompany"/>
      <rdfs:domain rdf:resource="&fibo-be-corp-corp;IncorporatedCompany"/>
      <rdfs:range rdf:resource="&fibo-be-corp-corp;IncorporatedCompany"/>
   </owl:ObjectProperty>

   <owl:ObjectProperty rdf:about="&fibo-be-oacx-ber;majorityVotingShareholdingBy">
      <rdfs:label>majority voting shareholding by</rdfs:label>
      <skos:definition>Formal Organization holding over fifty percent of the voting shares in this Incorporated Company.</skos:definition>
      <rdfs:subPropertyOf rdf:resource="&fibo-be-oacx-ber;someVotingShareholdingBy"/>
      <rdfs:subPropertyOf rdf:resource="&fibo-be-oacx-ber;majorityControllingInterestBy"/>
      <rdfs:domain rdf:resource="&fibo-be-corp-corp;IncorporatedCompany"/>
      <rdfs:range rdf:resource="&fibo-be-le-fbo;FormallyConstitutedOrganization"/>
   </owl:ObjectProperty>

   <owl:ObjectProperty rdf:about="&fibo-be-oacx-ber;partOwnedBy">
      <rdfs:label>part owned by</rdfs:label>
      <skos:definition>The entity is owned in some part by this kind of entity.</skos:definition>
      <rdfs:domain rdf:resource="&fibo-be-le-fbo;FormallyConstitutedOrganization"/>
      <rdfs:range rdf:resource="&fibo-fnd-pty-pty;IndependentParty"/>
   </owl:ObjectProperty>

   <owl:ObjectProperty rdf:about="&fibo-be-oacx-ber;significantControllingInterestBy">
      <rdfs:label>significant controlling interest by</rdfs:label>
      <skos:definition>Entity which has significant control of the Formal Organization.</skos:definition>
      <rdfs:domain rdf:resource="&fibo-be-le-fbo;FormallyConstitutedOrganization"/>
      <rdfs:range rdf:resource="&fibo-fnd-pty-pty;IndependentParty"/>
   </owl:ObjectProperty>

   <owl:ObjectProperty rdf:about="&fibo-be-oacx-ber;significantControllingInterestByCompany">
      <rdfs:label>significant controlling interest by company</rdfs:label>
      <skos:definition>Incorporated Company having a significant voting ownership in the Incorporated Company.</skos:definition>
      <rdfs:subPropertyOf rdf:resource="&fibo-be-oacx-ber;significantVotingShareholdingBy"/>
      <rdfs:subPropertyOf rdf:resource="&fibo-be-oacx-ber;someControllingInterestByCompany"/>
      <rdfs:domain rdf:resource="&fibo-be-corp-corp;IncorporatedCompany"/>
      <rdfs:range rdf:resource="&fibo-be-corp-corp;IncorporatedCompany"/>
   </owl:ObjectProperty>

   <owl:ObjectProperty rdf:about="&fibo-be-oacx-ber;significantVotingShareholdingBy">
      <rdfs:label>significant voting shareholding by</rdfs:label>
      <skos:definition>Formal Organization having significant voting ownership in the Incorporated Company.</skos:definition>
      <rdfs:subPropertyOf rdf:resource="&fibo-be-oacx-ber;significantControllingInterestBy"/>
      <rdfs:subPropertyOf rdf:resource="&fibo-be-oacx-ber;someVotingShareholdingBy"/>
      <rdfs:domain rdf:resource="&fibo-be-corp-corp;IncorporatedCompany"/>
      <rdfs:range rdf:resource="&fibo-be-le-fbo;FormallyConstitutedOrganization"/>
   </owl:ObjectProperty>

   <owl:ObjectProperty rdf:about="&fibo-be-oacx-ber;someControllingInterestByCompany">
      <rdfs:label>some controlling interest by company</rdfs:label>
      <skos:definition>Company having some degree of voting ownership in the company.</skos:definition>
      <rdfs:subPropertyOf rdf:resource="&fibo-be-oacx-ber;someVotingShareholdingBy"/>
      <rdfs:domain rdf:resource="&fibo-be-corp-corp;IncorporatedCompany"/>
      <rdfs:range rdf:resource="&fibo-be-corp-corp;IncorporatedCompany"/>
   </owl:ObjectProperty>

   <owl:ObjectProperty rdf:about="&fibo-be-oacx-ber;someVotingShareholdingBy">
      <rdfs:label>some voting shareholding by</rdfs:label>
      <skos:definition>Formal Organization having some degree of voting ownership in the company.</skos:definition>
      <rdfs:domain rdf:resource="&fibo-be-corp-corp;IncorporatedCompany"/>
      <rdfs:range rdf:resource="&fibo-be-le-fbo;FormallyConstitutedOrganization"/>
   </owl:ObjectProperty>

   <owl:ObjectProperty rdf:about="&fibo-be-oacx-ber;totalVotingShareholdingBy">
      <rdfs:label>total voting shareholding by</rdfs:label>
      <skos:definition>Formal Organization holding all of the voting shares in the Incorporated Company.</skos:definition>
      <rdfs:subPropertyOf rdf:resource="&fibo-be-oacx-ber;majorityVotingShareholdingBy"/>
      <rdfs:domain rdf:resource="&fibo-be-corp-corp;IncorporatedCompany"/>
      <rdfs:range rdf:resource="&fibo-be-le-fbo;FormallyConstitutedOrganization"/>
   </owl:ObjectProperty>

   <owl:ObjectProperty rdf:about="&fibo-be-oacx-ber;whollyControlledBy">
      <rdfs:label>wholly controlled by</rdfs:label>
      <skos:definition>Entity having controlling ownership of the Formal Organization.</skos:definition>
      <rdfs:subPropertyOf rdf:resource="&fibo-be-oacx-ber;legallyControlledBy"/>
      <rdfs:domain rdf:resource="&fibo-be-le-fbo;FormallyConstitutedOrganization"/>
      <rdfs:range rdf:resource="&fibo-fnd-pty-pty;IndependentParty"/>
   </owl:ObjectProperty>

   <owl:ObjectProperty rdf:about="&fibo-be-oacx-ber;whollyOwnedBy">
      <rdfs:label>wholly owned by</rdfs:label>
      <skos:definition>Incorporated Company holding all of the voting shares in the Incorporated Company.</skos:definition>
      <rdfs:subPropertyOf rdf:resource="&fibo-be-oacx-ber;majorityControllingOwnershipBy"/>
      <rdfs:subPropertyOf rdf:resource="&fibo-be-oacx-ber;totalVotingShareholdingBy"/>
      <rdfs:domain rdf:resource="&fibo-be-corp-corp;IncorporatedCompany"/>
      <rdfs:range rdf:resource="&fibo-be-corp-corp;IncorporatedCompany"/>
   </owl:ObjectProperty>


  <!--
    ///////////////////////////////////////////////////////////////////////////////////////
    //
    // Data Properties
    //
    ///////////////////////////////////////////////////////////////////////////////////////
    -->



  <!--
    ///////////////////////////////////////////////////////////////////////////////////////
    //
    // Annotation Properties
    //
    ///////////////////////////////////////////////////////////////////////////////////////
    -->



  <!--
    ///////////////////////////////////////////////////////////////////////////////////////
    //
    // Classes
    //
    ///////////////////////////////////////////////////////////////////////////////////////
    -->



  <!--
    ///////////////////////////////////////////////////////////////////////////////////////
    //
    // Individuals
    //
    ///////////////////////////////////////////////////////////////////////////////////////
    -->


</rdf:RDF>