<?xml version="1.0" encoding="UTF-8"?>
  
<!DOCTYPE rdf:RDF [
    <!ENTITY fibo-fnd-law-cor "http://spec.edmcouncil.org/fibo/red/fnd/law/legal-core/">
    <!ENTITY fibo-uo-lat "http://spec.edmcouncil.org/fibo/red/uo/lattice/">
    <!ENTITY fibo-fnd-rel-rel "http://spec.edmcouncil.org/fibo/red/fnd/relations/relations/">
    <!ENTITY fibo-fnd-org-fm "http://spec.edmcouncil.org/fibo/red/fnd/organizations/formal-organizations/">
    <!ENTITY fibo-uo-rl "http://spec.edmcouncil.org/fibo/red/uo/relatives/">
]>

<rdf:RDF xmlns:xsd="http://www.w3.org/2001/XMLSchema#"
         xmlns:sm="http://www.omg.org/techprocess/ab/SpecificationMetadata/"
         xmlns:xs="http://www.w3.org/2001/XMLSchema"
         xmlns:fibo-fnd-utl-av="http://www.omg.org/spec/EDMC-FIBO/FND/Utilities/AnnotationVocabulary/"
         xmlns:rdf="http://www.w3.org/1999/02/22-rdf-syntax-ns#"
         xmlns:rdfs="http://www.w3.org/2000/01/rdf-schema#"
         xmlns:owl="http://www.w3.org/2002/07/owl#"
         xmlns:skos="http://www.w3.org/2004/02/skos/core#"
         xmlns:dc="http://purl.org/dc/terms/"
         xml:base="http://spec.edmcouncil.org/fibo/red/fnd/law/legal-core/">

   <owl:Ontology rdf:about="http://spec.edmcouncil.org/fibo/red/fnd/law/legal-core/">
      <owl:imports rdf:resource="http://spec.edmcouncil.org/fibo/red/uo/lattice/"/>
      <owl:imports rdf:resource="http://spec.edmcouncil.org/fibo/red/fnd/relations/relations/"/>
      <owl:imports rdf:resource="http://spec.edmcouncil.org/fibo/red/fnd/organizations/formal-organizations/"/>
      <owl:imports rdf:resource="http://spec.edmcouncil.org/fibo/red/uo/relatives/"/>
   </owl:Ontology>


  <!--
    ///////////////////////////////////////////////////////////////////////////////////////
    //
    // Datatypes
    //
    ///////////////////////////////////////////////////////////////////////////////////////
    -->



  <!--
    ///////////////////////////////////////////////////////////////////////////////////////
    //
    // Object Properties
    //
    ///////////////////////////////////////////////////////////////////////////////////////
    -->


<owl:ObjectProperty rdf:about="&fibo-fnd-law-cor;governs">
      <rdfs:label>governs</rdfs:label>
      <skos:definition>The constitution governs and constrains the application of the or each body of law in the jurisdiction other framework to which it applies.</skos:definition>
      <rdfs:subPropertyOf rdf:resource="&fibo-fnd-rel-rel;governs"/>
      <rdfs:domain rdf:resource="&fibo-fnd-law-cor;Constitution"/>
      <rdfs:range rdf:resource="&fibo-fnd-law-cor;Law"/>
   </owl:ObjectProperty>


  <!--
    ///////////////////////////////////////////////////////////////////////////////////////
    //
    // Data Properties
    //
    ///////////////////////////////////////////////////////////////////////////////////////
    -->



  <!--
    ///////////////////////////////////////////////////////////////////////////////////////
    //
    // Annotation Properties
    //
    ///////////////////////////////////////////////////////////////////////////////////////
    -->



  <!--
    ///////////////////////////////////////////////////////////////////////////////////////
    //
    // Classes
    //
    ///////////////////////////////////////////////////////////////////////////////////////
    -->


<owl:Class rdf:about="&fibo-fnd-law-cor;Constitution">
      <rdfs:label>constitution</rdfs:label>
      <rdfs:subClassOf rdf:resource="&fibo-uo-lat;Concrete"/>
      <rdfs:subClassOf rdf:resource="&fibo-uo-lat;ContinuantThing"/>
      <rdfs:subClassOf rdf:resource="&fibo-uo-rl;IndependentThing"/>
   </owl:Class>

   <owl:Class rdf:about="&fibo-fnd-law-cor;CourtOfLaw">
      <rdfs:label>court of law</rdfs:label>
      <skos:definition>Some formal body with the mandate to hear disputes or cases.</skos:definition>
      <rdfs:subClassOf rdf:resource="&fibo-fnd-org-fm;FormalOrganization"/>
   </owl:Class>

   <owl:Class rdf:about="&fibo-fnd-law-cor;GovernmentalConstitution">
      <rdfs:label>governmental constitution</rdfs:label>
      <skos:definition>A body of rules, commitments and statements that set out how a country, state or territory is to be run.</skos:definition>
      <rdfs:subClassOf rdf:resource="&fibo-fnd-law-cor;Constitution"/>
   </owl:Class>

   <owl:Class rdf:about="&fibo-fnd-law-cor;Law">
      <rdfs:label>law</rdfs:label>
   </owl:Class>

   <owl:Class rdf:about="&fibo-fnd-law-cor;Ordinance">
      <rdfs:label>ordinance</rdfs:label>
      <skos:definition>An authoritative rule or law; a decree or command; a public injunction or regulation, such as a city ordinance against excessive horn blowing. (Source: Dictionary.com)</skos:definition>
      <rdfs:subClassOf rdf:resource="&fibo-fnd-law-cor;Law"/>
   </owl:Class>


  <!--
    ///////////////////////////////////////////////////////////////////////////////////////
    //
    // Individuals
    //
    ///////////////////////////////////////////////////////////////////////////////////////
    -->


</rdf:RDF>