<?xml version="1.0"?>


<!DOCTYPE rdf:RDF [
    <!ENTITY dct "http://purl.org/dc/terms/" >
    <!ENTITY owl "http://www.w3.org/2002/07/owl#" >
    <!ENTITY xsd "http://www.w3.org/2001/XMLSchema#" >
    <!ENTITY skos "http://www.w3.org/2004/02/skos/core#" >
    <!ENTITY rdfs "http://www.w3.org/2000/01/rdf-schema#" >
    <!ENTITY rdf "http://www.w3.org/1999/02/22-rdf-syntax-ns#" >
    <!ENTITY fibo-fnd-pty-rl "http://www.omg.org/spec/EDMC-FIBO/FND/Parties/Roles/" >
    <!ENTITY fibo-fnd-law-cor "http://www.omg.org/spec/EDMC-FIBO/FND/Law/LegalCore/" >
    <!ENTITY fibo-fnd-pty-pty "http://www.omg.org/spec/EDMC-FIBO/FND/Parties/Parties/" >
    <!ENTITY fibo-fnd-law-jur "http://www.omg.org/spec/EDMC-FIBO/FND/Law/Jurisdiction/" >
    <!ENTITY fibo-fnd-plc-loc "http://www.omg.org/spec/EDMC-FIBO/FND/Places/Locations/" >
    <!ENTITY fibo-fnd-plc-cty "http://www.omg.org/spec/EDMC-FIBO/FND/Places/Countries/" >
    <!ENTITY fibo-fnd-plc-adr "http://www.omg.org/spec/EDMC-FIBO/FND/Places/Addresses/" >
    <!ENTITY sm "http://www.omg.org/techprocess/ab/SpecificationMetadata/" >
    <!ENTITY fibo-fnd-rel-rel "http://www.omg.org/spec/EDMC-FIBO/FND/Relations/Relations/" >
    <!ENTITY fibo-fnd-agr-ctr "http://www.omg.org/spec/EDMC-FIBO/FND/Agreements/Contracts/" >
    <!ENTITY fibo-fnd-agr-agr "http://www.omg.org/spec/EDMC-FIBO/FND/Agreements/Agreements/" >
    <!ENTITY fibo-fnd-aap-agt "http://www.omg.org/spec/EDMC-FIBO/FND/AgentsAndPeople/Agents/" >
    <!ENTITY fibo-fnd-aap-ppl "http://www.omg.org/spec/EDMC-FIBO/FND/AgentsAndPeople/People/" >
    <!ENTITY fibo-fnd-gao-gl "http://www.omg.org/spec/EDMC-FIBO/FND/GoalsAndObjectives/Goals/" >
    <!ENTITY fibo-fnd-org-org "http://www.omg.org/spec/EDMC-FIBO/FND/Organizations/Organizations/" >
    <!ENTITY fibo-fnd-utl-bt "http://www.omg.org/spec/EDMC-FIBO/FND/Utilities/BusinessFacingTypes/" >
    <!ENTITY fibo-fnd-utl-av "http://www.omg.org/spec/EDMC-FIBO/FND/Utilities/AnnotationVocabulary/" >
    <!ENTITY fibo-fnd-org-fm "http://www.omg.org/spec/EDMC-FIBO/FND/Organizations/FormalOrganizations/" >
]>


<rdf:RDF xmlns="http://www.omg.org/spec/EDMC-FIBO/FND/Agreements/Contracts/"
     xml:base="http://www.omg.org/spec/EDMC-FIBO/FND/Agreements/Contracts/"
     xmlns:fibo-fnd-aap-agt="http://www.omg.org/spec/EDMC-FIBO/FND/AgentsAndPeople/Agents/"
     xmlns:fibo-fnd-pty-rl="http://www.omg.org/spec/EDMC-FIBO/FND/Parties/Roles/"
     xmlns:fibo-fnd-utl-bt="http://www.omg.org/spec/EDMC-FIBO/FND/Utilities/BusinessFacingTypes/"
     xmlns:fibo-fnd-agr-ctr="http://www.omg.org/spec/EDMC-FIBO/FND/Agreements/Contracts/"
     xmlns:fibo-fnd-law-cor="http://www.omg.org/spec/EDMC-FIBO/FND/Law/LegalCore/"
     xmlns:rdfs="http://www.w3.org/2000/01/rdf-schema#"
     xmlns:fibo-fnd-org-fm="http://www.omg.org/spec/EDMC-FIBO/FND/Organizations/FormalOrganizations/"
     xmlns:fibo-fnd-plc-cty="http://www.omg.org/spec/EDMC-FIBO/FND/Places/Countries/"
     xmlns:rdf="http://www.w3.org/1999/02/22-rdf-syntax-ns#"
     xmlns:fibo-fnd-aap-ppl="http://www.omg.org/spec/EDMC-FIBO/FND/AgentsAndPeople/People/"
     xmlns:sm="http://www.omg.org/techprocess/ab/SpecificationMetadata/"
     xmlns:fibo-fnd-plc-adr="http://www.omg.org/spec/EDMC-FIBO/FND/Places/Addresses/"
     xmlns:fibo-fnd-utl-av="http://www.omg.org/spec/EDMC-FIBO/FND/Utilities/AnnotationVocabulary/"
     xmlns:fibo-fnd-agr-agr="http://www.omg.org/spec/EDMC-FIBO/FND/Agreements/Agreements/"
     xmlns:fibo-fnd-pty-pty="http://www.omg.org/spec/EDMC-FIBO/FND/Parties/Parties/"
     xmlns:fibo-fnd-law-jur="http://www.omg.org/spec/EDMC-FIBO/FND/Law/Jurisdiction/"
     xmlns:fibo-fnd-rel-rel="http://www.omg.org/spec/EDMC-FIBO/FND/Relations/Relations/"
     xmlns:fibo-fnd-org-org="http://www.omg.org/spec/EDMC-FIBO/FND/Organizations/Organizations/"
     xmlns:fibo-fnd-plc-loc="http://www.omg.org/spec/EDMC-FIBO/FND/Places/Locations/"
     xmlns:fibo-fnd-gao-gl="http://www.omg.org/spec/EDMC-FIBO/FND/GoalsAndObjectives/Goals/"
     xmlns:dct="http://purl.org/dc/terms/"
     xmlns:owl="http://www.w3.org/2002/07/owl#"
     xmlns:xsd="http://www.w3.org/2001/XMLSchema#"
     xmlns:skos="http://www.w3.org/2004/02/skos/core#">
    <owl:Ontology rdf:about="http://www.omg.org/spec/EDMC-FIBO/FND/Agreements/Contracts/">
        <rdfs:label>Financial Industry Business Ontology (FIBO) Contracts Ontology</rdfs:label>
        <sm:moduleVersion rdf:datatype="&xsd;string">1.0</sm:moduleVersion>
        <sm:thisVersion rdf:datatype="&xsd;string">1.0 </sm:thisVersion>
        <sm:publicationDate rdf:datatype="&xsd;dateTime">2013-08-26T18:00:00</sm:publicationDate>
        <sm:contributor rdf:datatype="&xsd;string">Adaptive, Inc.</sm:contributor>
        <sm:moduleName rdf:datatype="&xsd;string">Agreements </sm:moduleName>
        <sm:filename rdf:datatype="&xsd;string">Contracts Ontology</sm:filename>
        <sm:copyright rdf:datatype="&xsd;string">Copyright (c) 2013 EDM Council, Inc.
Copyright (c) 2013 Object Management Group, Inc.</sm:copyright>
        <sm:submitter rdf:datatype="&xsd;string">EDM Council, Inc.</sm:submitter>
        <sm:keyword rdf:datatype="&xsd;string">FIBO</sm:keyword>
        <sm:familyAbbreviation rdf:datatype="&xsd;string">FIBO</sm:familyAbbreviation>
        <sm:specificationAbstract rdf:datatype="&xsd;string">FIBO Foundations is a set of business concepts which are intended to support the financial industry terms semantics presented in other FIBO specifications.  

The FIBO Foundations models define concepts which are not unique to the financial services industry. From these, financial industry terms in other FIBO specifications may be derived by extension. Terms are also included which may be referred to by properties of things in those specifications. FIBO Foundations therefore includes a number of basic terms about legal, contractual and organizational concepts, among others. </sm:specificationAbstract>
        <sm:specificationAbbreviation rdf:datatype="&xsd;string">FIBO-FND</sm:specificationAbbreviation>
        <sm:moduleAbbreviation rdf:datatype="&xsd;string">FIBO-FND-AGR</sm:moduleAbbreviation>
        <sm:keyword rdf:datatype="&xsd;string">Financial Industry Business Ontology</sm:keyword>
        <sm:familyTitle rdf:datatype="&xsd;string">Financial Industry Business Ontology (FIBO)</sm:familyTitle>
        <sm:specificationTitle rdf:datatype="&xsd;string">Financial Industry Business Ontology (FIBO) Foundations Specification</sm:specificationTitle>
        <sm:specificationVersionStatus rdf:datatype="&xsd;string">Request For Comments (RFC)</sm:specificationVersionStatus>
        <dct:license rdf:datatype="&xsd;string">The MIT License:  Permission is hereby granted, free of charge, to any person obtaining a copy of this software and associated documentation files (the &quot;Software&quot;), to deal in the Software without restriction, including without limitation the rights to use, copy, modify, merge, publish, distribute, sublicense, and/or sell copies of the Software, and to permit persons to whom the Software is furnished to do so, subject to the following conditions:

The copyright notice and this permission notice shall be included in all copies or substantial portions of the Software.

THE SOFTWARE IS PROVIDED &quot;AS IS&quot;, WITHOUT WARRANTY OF ANY KIND, EXPRESS OR IMPLIED, INCLUDING BUT NOT LIMITED TO THE WARRANTIES OF MERCHANTABILITY, FITNESS FOR A PARTICULAR PURPOSE
AND NONINFRINGEMENT.  IN NO EVENT SHALL THE AUTHORS OR COPYRIGHT HOLDERS BE LIABLE FOR ANY CLAIM, DAMAGES OR OTHER LIABILITY, WHETHER IN AN ACTION OF CONTRACT, TORT OR OTHERWISE, ARISING FROM, OUT OF OR IN CONNECTION WITH THE SOFTWARE OR THE USE OR OTHER DEALINGS IN THE SOFTWARE.</dct:license>
        <sm:familyAbstract rdf:datatype="&xsd;string">The content that comprises the Financial Industry Business Ontology (FIBO) is documentation, interpretable in formal logic, of the concepts represented by finance industry terms as used in official financial organization documents such as contracts, product/service specifications and governance and regulatory compliance documents.</sm:familyAbstract>
        <sm:contributor rdf:datatype="&xsd;string">Thematix Partners LLC</sm:contributor>
        <sm:moduleAbstract rdf:datatype="&xsd;string">This module includes ontologies describing agreements between parties and contracts that formalize those agreements.  These cover written and verbal contracts, including contracts which may be transferred from one party to another. The latter form the basis for financial securities contracts.  The Contracts ontology also describes fundamental properties of contracts such as contractual terms, contract parties and so on, many of which form the basis for more specialized financial industry concepts such as interest payment terms, bond issuers and so on.</sm:moduleAbstract>
        <sm:fileAbstract rdf:datatype="&xsd;string">This ontology defines concepts relating to contracts, for use in other FIBO ontology elements. These include written contracts which are the concrete evidence of agreements between parties, along with verbal contracts. Contracts are further broken down into bilateral and transferable contracts, the latter being the basis for most financial instruments. Properties of contracts are also defined, in particular contractual terms and contract parties. These concepts all form the basis of concepts in the financial services industry, for example interest payment terms are a kind of contract terms set, and security holders are a kind of contract counterparty.</sm:fileAbstract>
        <skos:historyNote rdf:datatype="&xsd;string">This version of the FIBO Foundations Specification was revised primarily to reflect comments received at the March 2013 OMG Technical Meeting in Reston and reflected in the Errata discussed at the June 2013 OMG Technical Meeting in Berlin. 

Revisions to FIBO Foundations are managed per the process outlined in the Policies and Procedures for OMG standards, with the intent to maintain backwards compatibility in the ontologies to the degree possible.
  
The RDF/XML serialized OWL for the Foundations ODM/OWL ontologies have been checked for syntactic errors and logical consistency with Protege 4 (http://protege.stanford.edu/), HermiT 1.3.7 (http://www.hermit-reasoner.com/) and Pellet 2.2 (http://clarkparsia.com/pellet/).</skos:historyNote>
        <skos:changeNote rdf:datatype="&xsd;string">This version of the ontology was revised in advance of the September 2013 New Brunswick, NJ meeting, as follows:
   (1) to use slash style URI/IRIss (also called 303 URIs, vs. hash style) as required to support server side processing 
   (2) to use version-independent IRIs for all definitions internally as opposed to version-specific IRIs
   (3) to change the file suffix from .owl to .rdf to increase usability in RDF tools
   (4) to use 4-level abbreviations and corresponding namespace prefixes for all FIBO ontologies, reflecting a family/specification/module/ontology structure
   (5) to incorporate changes to the specification metadata to support documentation at the family, specification, module, and ontology level, similar to the abbreviations.</skos:changeNote>
        <sm:fileAbbreviation rdf:datatype="&xsd;string">fibo-fnd-agr-ctr</sm:fileAbbreviation>
        <sm:topicArea rdf:datatype="&xsd;string">finance</sm:topicArea>
        <sm:technologyArea rdf:datatype="&xsd;string">formal semantics</sm:technologyArea>
        <sm:keyword rdf:datatype="&xsd;string">foundational vocabulary</sm:keyword>
        <sm:responsibleTaskForce rdf:datatype="&xsd;anyURI">http://fdtf.omg.org/</sm:responsibleTaskForce>
        <dct:license rdf:datatype="&xsd;anyURI">http://opensource.org/licenses/mit-license.php</dct:license>
        <sm:addressForComments rdf:datatype="&xsd;anyURI">http://www.omg.org/issues/</sm:addressForComments>
        <sm:familyURL rdf:datatype="&xsd;anyURI">http://www.omg.org/spec/EDMC-FIBO/</sm:familyURL>
        <sm:specificationURL rdf:datatype="&xsd;anyURI">http://www.omg.org/spec/EDMC-FIBO/FND/</sm:specificationURL>
        <sm:specificationVersionURL rdf:datatype="&xsd;anyURI">http://www.omg.org/spec/EDMC-FIBO/FND/1.0/</sm:specificationVersionURL>
        <owl:versionIRI rdf:datatype="&xsd;anyURI">http://www.omg.org/spec/EDMC-FIBO/FND/20130801/Agreements/Contracts/</owl:versionIRI>
        <sm:dependsOn rdf:datatype="&xsd;anyURI">http://www.omg.org/spec/EDMC-FIBO/FND/AgentsAndPeople/Agents/</sm:dependsOn>
        <sm:dependsOn rdf:datatype="&xsd;anyURI">http://www.omg.org/spec/EDMC-FIBO/FND/AgentsAndPeople/People/</sm:dependsOn>
        <sm:dependsOn rdf:datatype="&xsd;anyURI">http://www.omg.org/spec/EDMC-FIBO/FND/Agreements/Agreements/</sm:dependsOn>
        <sm:dependsOn rdf:datatype="&xsd;anyURI">http://www.omg.org/spec/EDMC-FIBO/FND/GoalsAndObjectives/Goals/</sm:dependsOn>
        <sm:dependsOn rdf:datatype="&xsd;anyURI">http://www.omg.org/spec/EDMC-FIBO/FND/Law/Jurisdiction/</sm:dependsOn>
        <sm:dependsOn rdf:datatype="&xsd;anyURI">http://www.omg.org/spec/EDMC-FIBO/FND/Law/LegalCore/</sm:dependsOn>
        <sm:dependsOn rdf:datatype="&xsd;anyURI">http://www.omg.org/spec/EDMC-FIBO/FND/Organizations/FormalOrganizations/</sm:dependsOn>
        <sm:dependsOn rdf:datatype="&xsd;anyURI">http://www.omg.org/spec/EDMC-FIBO/FND/Organizations/Organizations/</sm:dependsOn>
        <sm:dependsOn rdf:datatype="&xsd;anyURI">http://www.omg.org/spec/EDMC-FIBO/FND/Parties/Parties/</sm:dependsOn>
        <sm:dependsOn rdf:datatype="&xsd;anyURI">http://www.omg.org/spec/EDMC-FIBO/FND/Parties/Roles/</sm:dependsOn>
        <sm:dependsOn rdf:datatype="&xsd;anyURI">http://www.omg.org/spec/EDMC-FIBO/FND/Places/Addresses/</sm:dependsOn>
        <sm:dependsOn rdf:datatype="&xsd;anyURI">http://www.omg.org/spec/EDMC-FIBO/FND/Places/Countries/</sm:dependsOn>
        <sm:dependsOn rdf:datatype="&xsd;anyURI">http://www.omg.org/spec/EDMC-FIBO/FND/Places/Locations/</sm:dependsOn>
        <sm:dependsOn rdf:datatype="&xsd;anyURI">http://www.omg.org/spec/EDMC-FIBO/FND/Relations/Relations/</sm:dependsOn>
        <sm:dependsOn rdf:datatype="&xsd;anyURI">http://www.omg.org/spec/EDMC-FIBO/FND/Utilities/AnnotationVocabulary/</sm:dependsOn>
        <sm:dependsOn rdf:datatype="&xsd;anyURI">http://www.omg.org/spec/EDMC-FIBO/FND/Utilities/BusinessFacingTypes/</sm:dependsOn>
        <sm:priorVersion rdf:datatype="&xsd;anyURI">http://www.omg.org/spec/FIBO/Foundations/20130601/Agreements/Contracts.owl</sm:priorVersion>
        <sm:contentLanguage rdf:datatype="&xsd;anyURI">http://www.omg.org/spec/ODM/</sm:contentLanguage>
        <sm:dependsOn rdf:datatype="&xsd;anyURI">http://www.omg.org/techprocess/ab/SpecificationMetadata/</sm:dependsOn>
        <sm:contentLanguage rdf:datatype="&xsd;anyURI">http://www.w3.org/standards/techs/owl#w3c_all</sm:contentLanguage>
        <sm:keyword rdf:datatype="&xsd;string">ontology</sm:keyword>
        <sm:keyword rdf:datatype="&xsd;string">vocabulary</sm:keyword>
        <owl:imports rdf:resource="http://www.omg.org/spec/EDMC-FIBO/FND/AgentsAndPeople/Agents/"/>
        <owl:imports rdf:resource="http://www.omg.org/spec/EDMC-FIBO/FND/AgentsAndPeople/People/"/>
        <owl:imports rdf:resource="http://www.omg.org/spec/EDMC-FIBO/FND/Agreements/Agreements/"/>
        <owl:imports rdf:resource="http://www.omg.org/spec/EDMC-FIBO/FND/GoalsAndObjectives/Goals/"/>
        <owl:imports rdf:resource="http://www.omg.org/spec/EDMC-FIBO/FND/Law/Jurisdiction/"/>
        <owl:imports rdf:resource="http://www.omg.org/spec/EDMC-FIBO/FND/Law/LegalCore/"/>
        <owl:imports rdf:resource="http://www.omg.org/spec/EDMC-FIBO/FND/Organizations/FormalOrganizations/"/>
        <owl:imports rdf:resource="http://www.omg.org/spec/EDMC-FIBO/FND/Organizations/Organizations/"/>
        <owl:imports rdf:resource="http://www.omg.org/spec/EDMC-FIBO/FND/Parties/Parties/"/>
        <owl:imports rdf:resource="http://www.omg.org/spec/EDMC-FIBO/FND/Parties/Roles/"/>
        <owl:imports rdf:resource="http://www.omg.org/spec/EDMC-FIBO/FND/Places/Addresses/"/>
        <owl:imports rdf:resource="http://www.omg.org/spec/EDMC-FIBO/FND/Places/Countries/"/>
        <owl:imports rdf:resource="http://www.omg.org/spec/EDMC-FIBO/FND/Places/Locations/"/>
        <owl:imports rdf:resource="http://www.omg.org/spec/EDMC-FIBO/FND/Relations/Relations/"/>
        <owl:imports rdf:resource="http://www.omg.org/spec/EDMC-FIBO/FND/Utilities/AnnotationVocabulary/"/>
        <owl:imports rdf:resource="http://www.omg.org/spec/EDMC-FIBO/FND/Utilities/BusinessFacingTypes/"/>
        <owl:imports rdf:resource="http://www.omg.org/techprocess/ab/SpecificationMetadata/"/>
    </owl:Ontology>
    


    <!-- 
    ///////////////////////////////////////////////////////////////////////////////////////
    //
    // Object Properties
    //
    ///////////////////////////////////////////////////////////////////////////////////////
     -->

    


    <!-- http://www.omg.org/spec/EDMC-FIBO/FND/Agreements/Contracts/definesTermsFor -->

    <owl:ObjectProperty rdf:about="&fibo-fnd-agr-ctr;definesTermsFor">
        <skos:definition>the contract sets out the terms for the something</skos:definition>
        <skos:changeNote>added to support requirements in Business Entities, 2013-05-22</skos:changeNote>
        <rdfs:domain rdf:resource="&fibo-fnd-agr-ctr;Contract"/>
    </owl:ObjectProperty>
    


    <!-- http://www.omg.org/spec/EDMC-FIBO/FND/Agreements/Contracts/hasCounterparty -->

    <owl:ObjectProperty rdf:about="&fibo-fnd-agr-ctr;hasCounterparty">
        <rdfs:label>has counterparty</rdfs:label>
        <skos:definition>identifies a counterparty to a contract</skos:definition>
        <rdfs:domain rdf:resource="&fibo-fnd-agr-ctr;Contract"/>
        <rdfs:range rdf:resource="&fibo-fnd-agr-ctr;ContractCounterparty"/>
        <rdfs:subPropertyOf rdf:resource="&fibo-fnd-pty-pty;hasPartyInRole"/>
    </owl:ObjectProperty>
    


    <!-- http://www.omg.org/spec/EDMC-FIBO/FND/Agreements/Contracts/hasGoverningJurisdiction -->

    <owl:ObjectProperty rdf:about="&fibo-fnd-agr-ctr;hasGoverningJurisdiction">
        <rdfs:label>has governing jurisdiction</rdfs:label>
        <skos:editorialNote>As modeled, this relationship combines two slightly different senses in which a Jurisdiction may be named in some Contract: the jurisdiction under whose laws the contract is deemed to be in force, and the jurisdiction under which the parties agree to submit in the event of any dispute resolution. Scope Note: One thing to tease out is whether &quot;Dispute Resolution&quot; and other forms of &quot;Governing Law&quot; are one and the same thing or not. Dispute Resolution is uncontroversial, the question is whether there are other implications to Governing Law or if it&apos;s the same thing. For instance I may undertake to behave as though I were responsible to a particular authority i.e. a particular set of statutes.</skos:editorialNote>
        <skos:definition>identifies the jurisdiction governing the contract, as agreed by all parties. In a written contract this is generally identified, for example, as Governing Law, namely the jurisdiction in which any disputes arising from the contract are to be resolved.</skos:definition>
        <rdfs:domain rdf:resource="&fibo-fnd-agr-ctr;Contract"/>
        <rdfs:range rdf:resource="&fibo-fnd-law-jur;Jurisdiction"/>
        <rdfs:subPropertyOf rdf:resource="&fibo-fnd-rel-rel;isGovernedBy"/>
    </owl:ObjectProperty>
    


    <!-- http://www.omg.org/spec/EDMC-FIBO/FND/Agreements/Contracts/hasNonBindingTerms -->

    <owl:ObjectProperty rdf:about="&fibo-fnd-agr-ctr;hasNonBindingTerms">
        <rdfs:label>has non-binding terms</rdfs:label>
        <skos:definition>refers to terms that are included in the contract but are not considered binding. In other words, a breach of such terms in the future would not be considered to be a breach of the contract.</skos:definition>
        <rdfs:domain rdf:resource="&fibo-fnd-agr-ctr;Contract"/>
        <rdfs:range rdf:resource="&fibo-fnd-agr-ctr;NonBindingTermsSet"/>
        <rdfs:subPropertyOf rdf:resource="&fibo-fnd-agr-ctr;hasTerms"/>
    </owl:ObjectProperty>
    


    <!-- http://www.omg.org/spec/EDMC-FIBO/FND/Agreements/Contracts/hasPrincipal -->

    <owl:ObjectProperty rdf:about="&fibo-fnd-agr-ctr;hasPrincipal">
        <rdfs:label>has principal</rdfs:label>
        <skos:definition>identifies the main or principal party to a contract</skos:definition>
        <rdfs:domain rdf:resource="&fibo-fnd-agr-ctr;Contract"/>
        <rdfs:range rdf:resource="&fibo-fnd-agr-ctr;ContractPrincipal"/>
        <rdfs:subPropertyOf rdf:resource="&fibo-fnd-pty-pty;hasPartyInRole"/>
    </owl:ObjectProperty>
    


    <!-- http://www.omg.org/spec/EDMC-FIBO/FND/Agreements/Contracts/hasTerms -->

    <owl:ObjectProperty rdf:about="&fibo-fnd-agr-ctr;hasTerms">
        <rdfs:label>has terms</rdfs:label>
        <skos:definition>identifies a set of terms that form part of the contract. These are generally grouped for convenience as definitions, such as debt repayment terms, and may or may not equate to a formal clause, section, paragraph or other textual construct of the contract.</skos:definition>
        <rdfs:domain rdf:resource="&fibo-fnd-agr-ctr;Contract"/>
        <rdfs:range rdf:resource="&fibo-fnd-agr-ctr;ContractTermsSet"/>
        <rdfs:subPropertyOf rdf:resource="&fibo-fnd-rel-rel;has"/>
    </owl:ObjectProperty>
    


    <!-- http://www.omg.org/spec/EDMC-FIBO/FND/Agreements/Contracts/hasThirdParty -->

    <owl:ObjectProperty rdf:about="&fibo-fnd-agr-ctr;hasThirdParty">
        <rdfs:label>has third party</rdfs:label>
        <skos:definition>identifies a party which is not signatory to the party but has some role in the overall context defined by the contract.</skos:definition>
        <rdfs:domain rdf:resource="&fibo-fnd-agr-ctr;Contract"/>
        <rdfs:range rdf:resource="&fibo-fnd-agr-ctr;ContractThirdParty"/>
        <rdfs:subPropertyOf rdf:resource="&fibo-fnd-pty-pty;hasPartyInRole"/>
    </owl:ObjectProperty>
    


    <!-- http://www.omg.org/spec/EDMC-FIBO/FND/Agreements/Contracts/supersedes -->

    <owl:ObjectProperty rdf:about="&fibo-fnd-agr-ctr;supersedes">
        <rdfs:label>supersedes</rdfs:label>
        <skos:definition>The or any earlier contract which this written contract supersedes, whether that earlier contract is written or verbal or implied.</skos:definition>
        <rdfs:range rdf:resource="&fibo-fnd-agr-ctr;Contract"/>
        <rdfs:domain rdf:resource="&fibo-fnd-agr-ctr;WrittenContract"/>
    </owl:ObjectProperty>
    


    <!-- 
    ///////////////////////////////////////////////////////////////////////////////////////
    //
    // Data properties
    //
    ///////////////////////////////////////////////////////////////////////////////////////
     -->

    


    <!-- http://www.omg.org/spec/EDMC-FIBO/FND/Agreements/Contracts/isAssignable -->

    <owl:DatatypeProperty rdf:about="&fibo-fnd-agr-ctr;isAssignable">
        <skos:definition>indicates whether the contract and the rights thereunder may be assigned by one of the signatories to some other party</skos:definition>
        <rdfs:range rdf:resource="&fibo-fnd-utl-bt;yesOrNo"/>
    </owl:DatatypeProperty>
    


    <!-- 
    ///////////////////////////////////////////////////////////////////////////////////////
    //
    // Classes
    //
    ///////////////////////////////////////////////////////////////////////////////////////
     -->

    


    <!-- http://www.omg.org/spec/EDMC-FIBO/FND/Agreements/Contracts/BilateralContract -->

    <owl:Class rdf:about="&fibo-fnd-agr-ctr;BilateralContract">
        <rdfs:label>bilateral contract</rdfs:label>
        <rdfs:subClassOf rdf:resource="&fibo-fnd-agr-ctr;Contract"/>
        <rdfs:subClassOf>
            <owl:Restriction>
                <owl:onProperty rdf:resource="&fibo-fnd-pty-pty;hasPartyInRole"/>
                <owl:onClass rdf:resource="&fibo-fnd-pty-pty;PartyInRole"/>
                <owl:qualifiedCardinality rdf:datatype="&xsd;nonNegativeInteger">2</owl:qualifiedCardinality>
            </owl:Restriction>
        </rdfs:subClassOf>
        <skos:definition>A contract between two specific named parties. The rights and obligations pertaining to either party cannot be transferred to another party without prior written permission or a change to the contract itself.</skos:definition>
    </owl:Class>
    


    <!-- http://www.omg.org/spec/EDMC-FIBO/FND/Agreements/Contracts/ConditionsPrecedent -->

    <owl:Class rdf:about="&fibo-fnd-agr-ctr;ConditionsPrecedent">
        <rdfs:label>conditions precedent</rdfs:label>
        <rdfs:subClassOf rdf:resource="&fibo-fnd-agr-ctr;ContractTermsSet"/>
        <skos:definition>Conditions precedent on some obligation. These are conditions which would alter the Obligation as it is otherwise stated.</skos:definition>
        <skos:editorialNote>Introduced for ISDA Master Agreement. It is likely that the Conditions Precedent defined for OTC Derivatives Master Agreements are actually applicable more widely. However, they are defined within the ISDA terms for now. Modeling note / review question: Modeled as a kind of Terms Set, combining terms and conditions. Should consider whether terms and conditions are distinct (Condition would then be a separate archetype).</skos:editorialNote>
    </owl:Class>
    


    <!-- http://www.omg.org/spec/EDMC-FIBO/FND/Agreements/Contracts/Contract -->

    <owl:Class rdf:about="&fibo-fnd-agr-ctr;Contract">
        <rdfs:label>contract</rdfs:label>
        <rdfs:subClassOf>
            <owl:Restriction>
                <owl:onProperty rdf:resource="&fibo-fnd-agr-ctr;isAssignable"/>
                <owl:qualifiedCardinality rdf:datatype="&xsd;nonNegativeInteger">1</owl:qualifiedCardinality>
                <owl:onDataRange rdf:resource="&fibo-fnd-utl-bt;yesOrNo"/>
            </owl:Restriction>
        </rdfs:subClassOf>
        <rdfs:subClassOf>
            <owl:Restriction>
                <owl:onProperty rdf:resource="&fibo-fnd-pty-pty;hasPartyInRole"/>
                <owl:onClass rdf:resource="&fibo-fnd-pty-pty;PartyInRole"/>
                <owl:minQualifiedCardinality rdf:datatype="&xsd;nonNegativeInteger">2</owl:minQualifiedCardinality>
            </owl:Restriction>
        </rdfs:subClassOf>
        <rdfs:subClassOf>
            <owl:Restriction>
                <owl:onProperty rdf:resource="&fibo-fnd-rel-rel;hasEffectiveDate"/>
                <owl:qualifiedCardinality rdf:datatype="&xsd;nonNegativeInteger">1</owl:qualifiedCardinality>
                <owl:onDataRange rdf:resource="&xsd;dateTime"/>
            </owl:Restriction>
        </rdfs:subClassOf>
        <skos:definition>A voluntary, deliberate, and legally binding agreement between two or more competent parties. Contracts are usually written but may be spoken or implied, and generally have to do with employment, sale or lease, or tenancy.</skos:definition>
        <fibo-fnd-utl-av:definitionOrigin> http://www.businessdictionary.com/definition/contract.html</fibo-fnd-utl-av:definitionOrigin>
    </owl:Class>
    


    <!-- http://www.omg.org/spec/EDMC-FIBO/FND/Agreements/Contracts/ContractCounterparty -->

    <owl:Class rdf:about="&fibo-fnd-agr-ctr;ContractCounterparty">
        <rdfs:label>contract counterparty</rdfs:label>
        <rdfs:subClassOf rdf:resource="&fibo-fnd-pty-pty;PartyInRole"/>
        <skos:editorialNote>This term in Investopedia is named &quot;counterparty&quot; not &quot;contract counterparty&quot;. Can we simplify this to &quot;counterparty&quot;? (efk)</skos:editorialNote>
        <fibo-fnd-utl-av:definitionOrigin> http://www.investopedia.com/terms/c/counterparty.asp</fibo-fnd-utl-av:definitionOrigin>
        <skos:definition>A counterparty is the other party that participates in a financial transaction.  Every transaction must have a counterparty in order for the transaction to go through. More specifically, every buyer of an asset must be paired up with a seller that is willing to sell and vice versa.</skos:definition>
    </owl:Class>
    


    <!-- http://www.omg.org/spec/EDMC-FIBO/FND/Agreements/Contracts/ContractOriginator -->

    <owl:Class rdf:about="&fibo-fnd-agr-ctr;ContractOriginator">
        <rdfs:label>contract originator</rdfs:label>
        <rdfs:subClassOf rdf:resource="&fibo-fnd-agr-ctr;ContractPrincipal"/>
        <skos:definition>The party which originates the transferable contract and acts as the Principal in that contract regardless of the owner or counterparty.</skos:definition>
    </owl:Class>
    


    <!-- http://www.omg.org/spec/EDMC-FIBO/FND/Agreements/Contracts/ContractPrincipal -->

    <owl:Class rdf:about="&fibo-fnd-agr-ctr;ContractPrincipal">
        <rdfs:label>contract principal</rdfs:label>
        <rdfs:subClassOf rdf:resource="&fibo-fnd-pty-pty;PartyInRole"/>
        <fibo-fnd-utl-av:definitionOrigin> http://www.businessdictionary.com/definition/principal.html</fibo-fnd-utl-av:definitionOrigin>
        <skos:definition>The party identified as being the principal or first party to a contract, in the event that the contract distinguishes any party as the principal. In law, the principal is the party that has the primary responsibility in a liability or obligation, as opposed to an endorser, guarantor, or surety.</skos:definition>
    </owl:Class>
    


    <!-- http://www.omg.org/spec/EDMC-FIBO/FND/Agreements/Contracts/ContractTermsSet -->

    <owl:Class rdf:about="&fibo-fnd-agr-ctr;ContractTermsSet">
        <rdfs:label>contract terms set</rdfs:label>
        <rdfs:subClassOf rdf:resource="&fibo-fnd-agr-ctr;ContractualElement"/>
        <rdfs:subClassOf>
            <owl:Restriction>
                <owl:onProperty rdf:resource="&fibo-fnd-rel-rel;hasPart"/>
                <owl:allValuesFrom rdf:resource="&fibo-fnd-agr-ctr;ContractTermsSet"/>
            </owl:Restriction>
        </rdfs:subClassOf>
        <skos:editorialNote>The concept &quot;contract terms set&quot; does not exist in any dictionary I could find, however &quot;terms and conditions&quot; does, and could be used for this purpose. Can we change this to TermsAndConditions? If TermsAndConditions have parts, I would suggest creating a class called TermOrCondition, which would then provide the range for hasPart, and which could be specialized for various kinds of clauses, as appropriate.(efk)</skos:editorialNote>
        <skos:definition>The conditions of a contract include the terms and conditions that set the rights and obligations of the contracting parties when a contract is awarded or entered into.  These include general conditions which are common to all types of contracts, such as general and special arrangements, provisions, requirements, rules, specifications, and standards that form an integral part of an agreement or contract, as well as special conditions which are peculiar to a specific contract (such as, contract change conditions, payment conditions, price variation clauses, penalties).</skos:definition>
        <fibo-fnd-utl-av:definitionOrigin> http://www.businessdictionary.com/definition/conditions-of-contract.html</fibo-fnd-utl-av:definitionOrigin>
        <fibo-fnd-utl-av:definitionOrigin> http://www.businessdictionary.com/definition/terms-and-conditions.html</fibo-fnd-utl-av:definitionOrigin>
    </owl:Class>
    


    <!-- http://www.omg.org/spec/EDMC-FIBO/FND/Agreements/Contracts/ContractThirdParty -->

    <owl:Class rdf:about="&fibo-fnd-agr-ctr;ContractThirdParty">
        <rdfs:label>contract third party</rdfs:label>
        <rdfs:subClassOf rdf:resource="&fibo-fnd-pty-pty;PartyInRole"/>
        <skos:editorialNote>The concept &quot;contract third party&quot; does not exist in any dictionary I could find, however &quot;third-party&quot; does, and could be used for this purpose. Can we change this to ThirdParty? (efk)</skos:editorialNote>
        <skos:definition>Someone who may be indirectly involved but is not a principal party to an arrangement, contract, deal, lawsuit, or transaction.</skos:definition>
        <fibo-fnd-utl-av:definitionOrigin> http://www.businessdictionary.com/definition/third-party.html</fibo-fnd-utl-av:definitionOrigin>
    </owl:Class>
    


    <!-- http://www.omg.org/spec/EDMC-FIBO/FND/Agreements/Contracts/ContractualDefinition -->

    <owl:Class rdf:about="&fibo-fnd-agr-ctr;ContractualDefinition">
        <rdfs:label>contractual definition</rdfs:label>
        <rdfs:subClassOf rdf:resource="&fibo-fnd-agr-ctr;ContractualElement"/>
        <skos:definition>The definition of something in some contract or other legal instrument.</skos:definition>
        <skos:editorialNote>These are agreed definitions which are then referred to in terms in contracts or other legal instruments.</skos:editorialNote>
        <skos:editorialNote>The concept &quot;contractual definition&quot; does not exist in any dictionary I could find. Can we change this to ContractTermOrDefinition? (efk)</skos:editorialNote>
    </owl:Class>
    


    <!-- http://www.omg.org/spec/EDMC-FIBO/FND/Agreements/Contracts/ContractualElement -->

    <owl:Class rdf:about="&fibo-fnd-agr-ctr;ContractualElement">
        <rdfs:label>contractual element</rdfs:label>
        <skos:definition>Anything which relates to contracts.</skos:definition>
        <skos:editorialNote>The concept &quot;contractual element&quot; does not exist in any dictionary I could find. Can we change this to ContractElement? (efk)</skos:editorialNote>
    </owl:Class>
    


    <!-- http://www.omg.org/spec/EDMC-FIBO/FND/Agreements/Contracts/ContractualRelationship -->

    <owl:Class rdf:about="&fibo-fnd-agr-ctr;ContractualRelationship">
        <rdfs:label>contractual relationship</rdfs:label>
        <skos:definition>A contractual relationship is evidenced by (1) an offer, (2) acceptance of the offer, and a (3) valid (legal and valuable) consideration. Each party to a contract acquires rights and duties relative to the rights and duties of the other parties. However, while all parties may expect a fair benefit from the contract (otherwise courts may set it aside as inequitable) it does not follow that each party will benefit to an equal extent. Existence of contractual-relationship does not necessarily mean the contract is enforceable, or that it is not void (see void contract) or voidable (see voidable Contract).</skos:definition>
        <fibo-fnd-utl-av:definitionOrigin> http://www.businessdictionary.com/definition/contract.html</fibo-fnd-utl-av:definitionOrigin>
    </owl:Class>
    


    <!-- http://www.omg.org/spec/EDMC-FIBO/FND/Agreements/Contracts/NonBindingTermsSet -->

    <owl:Class rdf:about="&fibo-fnd-agr-ctr;NonBindingTermsSet">
        <rdfs:label>non-binding terms set</rdfs:label>
        <rdfs:subClassOf rdf:resource="&fibo-fnd-agr-ctr;ContractTermsSet"/>
        <skos:definition>Terms which do not have binding legal standing on the Issuer or Holder.</skos:definition>
    </owl:Class>
    


    <!-- http://www.omg.org/spec/EDMC-FIBO/FND/Agreements/Contracts/PromissoryNote -->

    <owl:Class rdf:about="&fibo-fnd-agr-ctr;PromissoryNote">
        <rdfs:label>promissory note</rdfs:label>
        <rdfs:subClassOf rdf:resource="&fibo-fnd-agr-ctr;WrittenContract"/>
        <fibo-fnd-utl-av:definitionOrigin> http://www.businessdictionary.com/definition/promissory-note.html</fibo-fnd-utl-av:definitionOrigin>
        <skos:definition>A promissory note is a written, signed, unconditional, and unsecured promise by one party (the maker or promisor) to another (the payee or promisee) that commits the maker to pay a specified sum on demand, or on a fixed or a determinable date. Promissory notes (such as bank or currency notes) are negotiable instruments.</skos:definition>
        <skos:editorialNote>Unlike a contract, a Promissory Note does not need to be signed by both parties. It is essentiually a promise from one party to the holder, of some good or benefit. Promissory notes would generally by fully fungible. These are modeled as a kind of contract but are essentially a kind of unilateral contract between the issuer and the holder, and some authorities might not see this as a contract at all. Cash is a kind of promissory note, with the issuer being a central bank.</skos:editorialNote>
    </owl:Class>
    


    <!-- http://www.omg.org/spec/EDMC-FIBO/FND/Agreements/Contracts/TransferableContract -->

    <owl:Class rdf:about="&fibo-fnd-agr-ctr;TransferableContract">
        <rdfs:label>transferable contract</rdfs:label>
        <owl:equivalentClass>
            <owl:Restriction>
                <owl:onProperty rdf:resource="&fibo-fnd-agr-ctr;hasPrincipal"/>
                <owl:onClass rdf:resource="&fibo-fnd-agr-ctr;ContractOriginator"/>
                <owl:minQualifiedCardinality rdf:datatype="&xsd;nonNegativeInteger">1</owl:minQualifiedCardinality>
            </owl:Restriction>
        </owl:equivalentClass>
        <rdfs:subClassOf rdf:resource="&fibo-fnd-agr-ctr;WrittenContract"/>
        <rdfs:subClassOf>
            <owl:Restriction>
                <owl:onProperty rdf:resource="&fibo-fnd-agr-ctr;hasCounterparty"/>
                <owl:onClass rdf:resource="&fibo-fnd-agr-ctr;TransferableContractHolder"/>
                <owl:minQualifiedCardinality rdf:datatype="&xsd;nonNegativeInteger">1</owl:minQualifiedCardinality>
            </owl:Restriction>
        </rdfs:subClassOf>
        <fibo-fnd-utl-av:definitionOrigin>http://en.wikipedia.org/wiki/Assignment_(law)</fibo-fnd-utl-av:definitionOrigin>
        <skos:definition>An assignment (Latin cessio) is a term used with similar meanings in the law of contracts and in the law of real estate. In both instances, it encompasses the transfer of rights held by one party, the assignor, to another party, the assignee. The details of the assignment determines some additional rights and liabilities (or duties). Typically a third-party is involved in a contract with the assignor, and the contract is in effect transferred to the assignee.</skos:definition>
    </owl:Class>
    


    <!-- http://www.omg.org/spec/EDMC-FIBO/FND/Agreements/Contracts/TransferableContractHolder -->

    <owl:Class rdf:about="&fibo-fnd-agr-ctr;TransferableContractHolder">
        <rdfs:label>transferable contract holder</rdfs:label>
        <rdfs:subClassOf rdf:resource="&fibo-fnd-agr-ctr;ContractCounterparty"/>
        <skos:definition>The party which holds a transferable contract and enjoys the benefits defined in that contract while they hold it.</skos:definition>
        <skos:editorialNote>This party may transfer the contract to another party without reference to the issuer, for example by selling it in some marketplace.</skos:editorialNote>
    </owl:Class>
    


    <!-- http://www.omg.org/spec/EDMC-FIBO/FND/Agreements/Contracts/VerbalContract -->

    <owl:Class rdf:about="&fibo-fnd-agr-ctr;VerbalContract">
        <rdfs:label>verbal contract</rdfs:label>
        <rdfs:subClassOf rdf:resource="&fibo-fnd-agr-ctr;Contract"/>
        <owl:disjointWith rdf:resource="&fibo-fnd-agr-ctr;WrittenContract"/>
        <skos:definition>A contract which exists as a result of some verbal exchange.</skos:definition>
    </owl:Class>
    


    <!-- http://www.omg.org/spec/EDMC-FIBO/FND/Agreements/Contracts/WrittenContract -->

    <owl:Class rdf:about="&fibo-fnd-agr-ctr;WrittenContract">
        <rdfs:label>written contract</rdfs:label>
        <rdfs:subClassOf rdf:resource="&fibo-fnd-agr-ctr;Contract"/>
        <skos:definition>A formal Contract which is written and signed by both parties thereto.</skos:definition>
    </owl:Class>
</rdf:RDF>



<!-- Generated by the OWL API (version 3.4.2) http://owlapi.sourceforge.net -->

