<?xml version="1.0" encoding="UTF-8"?>
<!DOCTYPE rdf:RDF [
	<!ENTITY fibo-fnd-aap-agt "https://spec.edmcouncil.org/fibo/FND/AgentsAndPeople/Agents/">
	<!ENTITY fibo-fnd-inf-idx "https://spec.edmcouncil.org/fibo/FND/Information/Identifiers/">
	<!ENTITY fibo-fnd-inf-inf "https://spec.edmcouncil.org/fibo/FND/Information/InfoCore/">
	<!ENTITY fibo-fnd-inf-sch "https://spec.edmcouncil.org/fibo/FND/Information/Schemes/">
	<!ENTITY fibo-fnd-plc-cty "https://spec.edmcouncil.org/fibo/FND/Places/Countries/">
	<!ENTITY fibo-fnd-utl-av "https://spec.edmcouncil.org/fibo/FND/Utilities/AnnotationVocabulary/">
	<!ENTITY fibo-fnd-utlx-val "https://spec.edmcouncil.org/fibo/FND/UtilitiesExt/Values/">
	<!ENTITY fibo-uo-lat "https://spec.edmcouncil.org/fibo/UO/Lattice/">
	<!ENTITY owl "http://www.w3.org/2002/07/owl#">
	<!ENTITY rdf "http://www.w3.org/1999/02/22-rdf-syntax-ns#">
	<!ENTITY rdfs "http://www.w3.org/2000/01/rdf-schema#">
	<!ENTITY skos "http://www.w3.org/2004/02/skos/core#">
	<!ENTITY sm "http://www.omg.org/techprocess/ab/SpecificationMetadata/">
	<!ENTITY xsd "http://www.w3.org/2001/XMLSchema#">
]>
<rdf:RDF xml:base="https://spec.edmcouncil.org/fibo/FND/Information/Schemes/"
	xmlns:fibo-fnd-aap-agt="https://spec.edmcouncil.org/fibo/FND/AgentsAndPeople/Agents/"
	xmlns:fibo-fnd-inf-idx="https://spec.edmcouncil.org/fibo/FND/Information/Identifiers/"
	xmlns:fibo-fnd-inf-inf="https://spec.edmcouncil.org/fibo/FND/Information/InfoCore/"
	xmlns:fibo-fnd-inf-sch="https://spec.edmcouncil.org/fibo/FND/Information/Schemes/"
	xmlns:fibo-fnd-plc-cty="https://spec.edmcouncil.org/fibo/FND/Places/Countries/"
	xmlns:fibo-fnd-utl-av="https://spec.edmcouncil.org/fibo/FND/Utilities/AnnotationVocabulary/"
	xmlns:fibo-fnd-utlx-val="https://spec.edmcouncil.org/fibo/FND/UtilitiesExt/Values/"
	xmlns:fibo-uo-lat="https://spec.edmcouncil.org/fibo/UO/Lattice/"
	xmlns:owl="http://www.w3.org/2002/07/owl#"
	xmlns:rdf="http://www.w3.org/1999/02/22-rdf-syntax-ns#"
	xmlns:rdfs="http://www.w3.org/2000/01/rdf-schema#"
	xmlns:skos="http://www.w3.org/2004/02/skos/core#"
	xmlns:sm="http://www.omg.org/techprocess/ab/SpecificationMetadata/"
	xmlns:xsd="http://www.w3.org/2001/XMLSchema#">
	
	<owl:Ontology rdf:about="https://spec.edmcouncil.org/fibo/FND/Information/Schemes/">
		<rdfs:label xml:lang="en">Schemes</rdfs:label>
		<owl:imports rdf:resource="http://www.omg.org/techprocess/ab/SpecificationMetadata/"/>
		<owl:imports rdf:resource="http://www.w3.org/2004/02/skos/core"/>
		<owl:imports rdf:resource="https://spec.edmcouncil.org/fibo/FND/AgentsAndPeople/Agents/"/>
		<owl:imports rdf:resource="https://spec.edmcouncil.org/fibo/FND/Information/Identifiers/"/>
		<owl:imports rdf:resource="https://spec.edmcouncil.org/fibo/FND/Information/InfoCore/"/>
		<owl:imports rdf:resource="https://spec.edmcouncil.org/fibo/FND/Places/Countries/"/>
		<owl:imports rdf:resource="https://spec.edmcouncil.org/fibo/FND/Utilities/AnnotationVocabulary/"/>
		<owl:imports rdf:resource="https://spec.edmcouncil.org/fibo/FND/UtilitiesExt/Values/"/>
		<fibo-fnd-utl-av:hasMaturityLevel rdf:resource="&fibo-fnd-utl-av;Informative"/>
	</owl:Ontology>
	
	<owl:Class rdf:about="&fibo-fnd-inf-sch;BusinessCalendarCode">
		<rdfs:subClassOf rdf:resource="&fibo-fnd-inf-sch;SchematicCode"/>
		<rdfs:label xml:lang="en">business calendar code</rdfs:label>
		<skos:definition xml:lang="en">The Calendar for a particular business center, which defines what are the working days in that center.</skos:definition>
		<fibo-fnd-utl-av:explanatoryNote xml:lang="en">This is the identification code for the calendar, not the calendar of dates itself. This code uniquely identifies the business calendar in which business days are defined. This is usually published year on year, but formal terms only need to identify the Calendar so that events are understood to be specified in terms of that calendar.</fibo-fnd-utl-av:explanatoryNote>
	</owl:Class>
	
	<owl:Class rdf:about="&fibo-fnd-inf-sch;BusinessCalendarScheme">
		<rdfs:subClassOf rdf:resource="&fibo-fnd-inf-sch;Scheme"/>
		<rdfs:subClassOf>
			<owl:Restriction>
				<owl:onProperty rdf:resource="&fibo-fnd-inf-sch;defines.1"/>
				<owl:someValuesFrom rdf:resource="&fibo-fnd-inf-sch;BusinessCalendarCode"/>
			</owl:Restriction>
		</rdfs:subClassOf>
		<rdfs:label xml:lang="en">business calendar scheme</rdfs:label>
	</owl:Class>
	
	<owl:Class rdf:about="&fibo-fnd-inf-sch;Classification">
		<rdfs:subClassOf rdf:resource="&fibo-fnd-inf-sch;SchematicCode"/>
		<rdfs:label xml:lang="en">classification</rdfs:label>
		<skos:definition xml:lang="en">Some Classification of some Thing to identify what type of Thing it is (usually within a particular class of Things such as financial securities or organisations).</skos:definition>
	</owl:Class>
	
	<owl:Class rdf:about="&fibo-fnd-inf-sch;ClassificationScheme">
		<rdfs:subClassOf rdf:resource="&fibo-fnd-inf-sch;Scheme"/>
		<rdfs:subClassOf>
			<owl:Restriction>
				<owl:onProperty rdf:resource="&fibo-fnd-inf-sch;defines.1"/>
				<owl:someValuesFrom rdf:resource="&fibo-fnd-inf-sch;Classification"/>
			</owl:Restriction>
		</rdfs:subClassOf>
		<rdfs:label xml:lang="en">classification scheme</rdfs:label>
		<skos:definition xml:lang="en">The Scheme defining how the Classification is determined. This may be a URI or some other unique identification of the Scheme.</skos:definition>
	</owl:Class>
	
	<owl:Class rdf:about="&fibo-fnd-inf-sch;CountryCode">
		<rdfs:subClassOf rdf:resource="&fibo-fnd-inf-idx;Identifier"/>
		<rdfs:subClassOf>
			<owl:Restriction>
				<owl:onProperty rdf:resource="&fibo-fnd-inf-idx;uniquelyIdentifies"/>
				<owl:someValuesFrom rdf:resource="&fibo-fnd-plc-cty;Country"/>
			</owl:Restriction>
		</rdfs:subClassOf>
		<rdfs:label xml:lang="en">country code</rdfs:label>
		<skos:definition xml:lang="en">A recognized, standardized code by which a country can be uniquely identified.</skos:definition>
	</owl:Class>
	
	<owl:Class rdf:about="&fibo-fnd-inf-sch;CountryCodeScheme">
		<rdfs:subClassOf rdf:resource="&fibo-fnd-inf-idx;IdentificationScheme"/>
		<rdfs:subClassOf>
			<owl:Restriction>
				<owl:onProperty rdf:resource="&fibo-fnd-inf-sch;defines.1"/>
				<owl:someValuesFrom rdf:resource="&fibo-fnd-inf-sch;CountryCode"/>
			</owl:Restriction>
		</rdfs:subClassOf>
		<rdfs:label xml:lang="en">country code scheme</rdfs:label>
	</owl:Class>
	
	<owl:Class rdf:about="&fibo-fnd-inf-sch;CurrencyCode">
		<rdfs:subClassOf rdf:resource="&fibo-fnd-inf-sch;SchematicCode"/>
		<rdfs:label xml:lang="en">currency code</rdfs:label>
	</owl:Class>
	
	<owl:Class rdf:about="&fibo-fnd-inf-sch;CurrencyCodeScheme">
		<rdfs:subClassOf rdf:resource="&fibo-fnd-inf-sch;Scheme"/>
		<rdfs:subClassOf>
			<owl:Restriction>
				<owl:onProperty rdf:resource="&fibo-fnd-inf-sch;defines.1"/>
				<owl:someValuesFrom rdf:resource="&fibo-fnd-inf-sch;CurrencyCode"/>
			</owl:Restriction>
		</rdfs:subClassOf>
		<rdfs:label xml:lang="en">currency code scheme</rdfs:label>
	</owl:Class>
	
	<owl:Class rdf:about="&fibo-fnd-inf-sch;RegistrationCode">
		<rdfs:subClassOf rdf:resource="&fibo-fnd-inf-inf;Information"/>
		<rdfs:label xml:lang="en">registration code</rdfs:label>
		<skos:definition xml:lang="en">Any code by which something in formally registered, for example for the purposes of legal identification.</skos:definition>
	</owl:Class>
	
	<owl:Class rdf:about="&fibo-fnd-inf-sch;SchematicCode">
		<rdfs:subClassOf rdf:resource="&fibo-fnd-inf-inf;Information"/>
		<rdfs:subClassOf>
			<owl:Restriction>
				<owl:onProperty rdf:resource="&fibo-fnd-inf-sch;definedIn"/>
				<owl:someValuesFrom rdf:resource="&fibo-fnd-inf-sch;Scheme"/>
			</owl:Restriction>
		</rdfs:subClassOf>
		<rdfs:label xml:lang="en">schematic code</rdfs:label>
		<skos:definition xml:lang="en">A code which is defined in some scheme as having some meaning.</skos:definition>
		<fibo-fnd-utl-av:explanatoryNote xml:lang="en">It is assumed that, even though this may sometimes be defined in the relevant scheme as a numerical value, this can be treated universally as a text code. Otherwise each individual kind of code would have to have some definition of whether it is necessarily code or numeric, which makes no sense. Where schemes are numeric, this is treated as a text because its meaning is defined in a scheme and so is not in any sense a number.</fibo-fnd-utl-av:explanatoryNote>
	</owl:Class>
	
	<owl:Class rdf:about="&fibo-fnd-inf-sch;Scheme">
		<rdfs:subClassOf rdf:resource="&fibo-fnd-inf-inf;Information"/>
		<rdfs:subClassOf>
			<owl:Restriction>
				<owl:onProperty rdf:resource="&fibo-fnd-inf-sch;defines.1"/>
				<owl:someValuesFrom rdf:resource="&fibo-fnd-inf-sch;SchematicCode"/>
			</owl:Restriction>
		</rdfs:subClassOf>
		<rdfs:label xml:lang="en">scheme</rdfs:label>
		<skos:definition xml:lang="en">The scheme by which the schematic code is identified.</skos:definition>
	</owl:Class>
	
	<owl:ObjectProperty rdf:about="&fibo-fnd-inf-sch;classifies">
		<rdfs:subPropertyOf rdf:resource="&fibo-fnd-inf-inf;isAbout"/>
		<rdfs:label xml:lang="en">classifies red</rdfs:label>
		<rdfs:domain rdf:resource="&fibo-fnd-inf-sch;Classification"/>
		<skos:definition xml:lang="en">The thing which is classified by the classification code. This may be any independent thing, concrete or abstract and continuant or occurrent.</skos:definition>
	</owl:ObjectProperty>
	
	<owl:ObjectProperty rdf:about="&fibo-fnd-inf-sch;code">
		<rdfs:label xml:lang="en">code</rdfs:label>
		<rdfs:label xml:lang="en">has code</rdfs:label>
		<rdfs:domain rdf:resource="&fibo-fnd-inf-sch;SchematicCode"/>
		<rdfs:range rdf:resource="&fibo-fnd-utlx-val;TextValue"/>
	</owl:ObjectProperty>
	
	<owl:ObjectProperty rdf:about="&fibo-fnd-inf-sch;definedIn">
		<rdfs:label xml:lang="en">defined in</rdfs:label>
		<rdfs:domain rdf:resource="&fibo-fnd-inf-sch;SchematicCode"/>
		<rdfs:range rdf:resource="&fibo-fnd-inf-sch;Scheme"/>
		<owl:inverseOf rdf:resource="&fibo-fnd-inf-sch;defines.1"/>
	</owl:ObjectProperty>
	
	<owl:ObjectProperty rdf:about="&fibo-fnd-inf-sch;defines.1">
		<rdfs:label xml:lang="en">defines red</rdfs:label>
		<rdfs:domain rdf:resource="&fibo-fnd-inf-sch;Scheme"/>
		<rdfs:range rdf:resource="&fibo-fnd-inf-sch;SchematicCode"/>
		<skos:definition xml:lang="en">The scheme sets out the nature, structure and requirements of a set of Schematic Codes.</skos:definition>
	</owl:ObjectProperty>
	
	<owl:ObjectProperty rdf:about="&fibo-fnd-inf-sch;schemeReference">
		<rdfs:label xml:lang="en">scheme reference</rdfs:label>
		<rdfs:domain rdf:resource="&fibo-fnd-inf-sch;Scheme"/>
		<rdfs:range rdf:resource="&fibo-fnd-utlx-val;TextValue"/>
		<skos:definition xml:lang="en">The reference by which the scheme is identified, such as a URI.</skos:definition>
	</owl:ObjectProperty>
	
	<owl:Class rdf:about="&fibo-fnd-plc-cty;Country">
		<rdfs:subClassOf>
			<owl:Restriction>
				<owl:onProperty rdf:resource="&fibo-fnd-inf-idx;hasIdentifier"/>
				<owl:someValuesFrom rdf:resource="&fibo-fnd-inf-sch;CountryCode"/>
			</owl:Restriction>
		</rdfs:subClassOf>
		<rdfs:label xml:lang="en">country</rdfs:label>
		<owl:equivalentClass rdf:resource="&fibo-fnd-plc-cty;Country"/>
	</owl:Class>

</rdf:RDF>