<?xml version="1.0" encoding="UTF-8"?>
  
<!DOCTYPE rdf:RDF [
    <!ENTITY fibo-be-fct-fct "http://spec.edmcouncil.org/fibo/red/be/functional-entities/functional-entities/">
    <!ENTITY fibo-rl-rbe "http://spec.edmcouncil.org/fibo/red/fnd/relative/relative-business-entities/">
    <!ENTITY fibo-fnd-rel-rel "http://spec.edmcouncil.org/fibo/red/fnd/relations/relations/">
    <!ENTITY fibo-fnd-aap-agt "http://spec.edmcouncil.org/fibo/red/fnd/agents-and-people/agents/">
    <!ENTITY fibo-fnd-oac-own "http://spec.edmcouncil.org/fibo/red/fnd/ownership-and-control/ownership/">
    <!ENTITY fibo-be-le-fbo "http://spec.edmcouncil.org/fibo/red/be/legal-entities/formal-business-organizations/">
    <!ENTITY fibo-be-corp-corp "http://spec.edmcouncil.org/fibo/red/be/corporations/corporations/">
    <!ENTITY fibo-uo-rl "http://spec.edmcouncil.org/fibo/red/uo/relatives/">
    <!ENTITY fibo-be-le-lp "http://spec.edmcouncil.org/fibo/red/be/legal-entities/legal-persons/">
]>

<rdf:RDF xmlns:xsd="http://www.w3.org/2001/XMLSchema#"
         xmlns:sm="http://www.omg.org/techprocess/ab/SpecificationMetadata/"
         xmlns:xs="http://www.w3.org/2001/XMLSchema"
         xmlns:fibo-fnd-utl-av="http://www.omg.org/spec/EDMC-FIBO/FND/Utilities/AnnotationVocabulary/"
         xmlns:rdf="http://www.w3.org/1999/02/22-rdf-syntax-ns#"
         xmlns:rdfs="http://www.w3.org/2000/01/rdf-schema#"
         xmlns:owl="http://www.w3.org/2002/07/owl#"
         xmlns:skos="http://www.w3.org/2004/02/skos/core#"
         xmlns:dc="http://purl.org/dc/terms/"
         xml:base="http://spec.edmcouncil.org/fibo/red/be/functional-entities/functional-entities/">

   <owl:Ontology rdf:about="http://spec.edmcouncil.org/fibo/red/be/functional-entities/functional-entities/">
      <owl:imports rdf:resource="http://spec.edmcouncil.org/fibo/red/fnd/relative/relative-business-entities/"/>
      <owl:imports rdf:resource="http://spec.edmcouncil.org/fibo/red/fnd/relations/relations/"/>
      <owl:imports rdf:resource="http://spec.edmcouncil.org/fibo/red/fnd/agents-and-people/agents/"/>
      <owl:imports rdf:resource="http://spec.edmcouncil.org/fibo/red/fnd/ownership-and-control/ownership/"/>
      <owl:imports rdf:resource="http://spec.edmcouncil.org/fibo/red/be/legal-entities/formal-business-organizations/"/>
      <owl:imports rdf:resource="http://spec.edmcouncil.org/fibo/red/be/corporations/corporations/"/>
      <owl:imports rdf:resource="http://spec.edmcouncil.org/fibo/red/uo/relatives/"/>
      <owl:imports rdf:resource="http://spec.edmcouncil.org/fibo/red/be/legal-entities/legal-persons/"/>
   </owl:Ontology>


  <!--
    ///////////////////////////////////////////////////////////////////////////////////////
    //
    // Datatypes
    //
    ///////////////////////////////////////////////////////////////////////////////////////
    -->



  <!--
    ///////////////////////////////////////////////////////////////////////////////////////
    //
    // Object Properties
    //
    ///////////////////////////////////////////////////////////////////////////////////////
    -->


<owl:ObjectProperty rdf:about="&fibo-be-fct-fct;benefitCorporationTakesForm">
      <rdfs:label>benefit corporation takes form</rdfs:label>
      <skos:definition>he Benefit Corporation takes the legal form of an Incorporated Company.</skos:definition>
      <rdfs:subPropertyOf rdf:resource="&fibo-be-fct-fct;functionalBusinessEntityTakesForm"/>
      <rdfs:domain rdf:resource="&fibo-be-fct-fct;BenefitCorporation"/>
      <rdfs:range rdf:resource="&fibo-be-corp-corp;IncorporatedCompany"/>
   </owl:ObjectProperty>

   <owl:ObjectProperty rdf:about="&fibo-be-fct-fct;businessIsCharacterizedBy">
      <rdfs:label>business is characterized by</rdfs:label>
      <skos:definition>A business is some entity which engages in some Commercial Activity.</skos:definition>
      <rdfs:subPropertyOf rdf:resource="&fibo-be-fct-fct;isCharacterizedBy"/>
      <rdfs:domain rdf:resource="&fibo-be-fct-fct;Business"/>
      <rdfs:range rdf:resource="&fibo-be-fct-fct;CommercialActivity"/>
   </owl:ObjectProperty>

   <owl:ObjectProperty rdf:about="&fibo-be-fct-fct;functionalBusinessEntityTakesForm">
      <rdfs:label>functional business entity takes form</rdfs:label>
      <skos:definition>The form which a Functional Business Entity takes. This may be any Autonomous Agent.</skos:definition>
      <rdfs:subPropertyOf rdf:resource="&fibo-rl-rbe;takesEntityForm"/>
      <rdfs:subPropertyOf rdf:resource="&fibo-fnd-oac-own;takesForm"/>
      <rdfs:domain rdf:resource="&fibo-be-fct-fct;FunctionalBusinessEntity"/>
      <rdfs:range rdf:resource="&fibo-fnd-aap-agt;AutonomousAgent"/>
   </owl:ObjectProperty>

   <owl:ObjectProperty rdf:about="&fibo-be-fct-fct;merchantIsCharacterizedBy">
      <rdfs:label>merchant is characterized by</rdfs:label>
      <skos:definition>The activity for which the Merchant is set up, is commerce, that is the purchase and sale of goods.</skos:definition>
      <rdfs:subPropertyOf rdf:resource="&fibo-be-fct-fct;businessIsCharacterizedBy"/>
      <rdfs:domain rdf:resource="&fibo-be-fct-fct;Merchant"/>
      <rdfs:range rdf:resource="&fibo-be-fct-fct;Commerce"/>
   </owl:ObjectProperty>

   <owl:ObjectProperty rdf:about="&fibo-be-fct-fct;nonProfitTakesForm">
      <rdfs:label>non profit takes form</rdfs:label>
      <skos:definition>A non profit or charitable public or private foundation takes the form of a legal entity. Further Notes Per Wikipedia it is necessarily a Legal Entity. "Foundation" is this a kind of legal entity separate from the ones already defined, or another word for a kind of functional entity? Definitin Origin:Wikipedia adapted</skos:definition>
      <rdfs:subPropertyOf rdf:resource="&fibo-be-fct-fct;functionalBusinessEntityTakesForm"/>
      <rdfs:domain rdf:resource="&fibo-be-fct-fct;NonProfitOrganization"/>
      <rdfs:range rdf:resource="&fibo-be-le-fbo;FormallyConstitutedOrganization"/>
   </owl:ObjectProperty>

   <owl:ObjectProperty rdf:about="&fibo-be-fct-fct;soleProprietorshipTakesForm">
      <rdfs:label>sole proprietorship takes form</rdfs:label>
      <skos:definition>The person who is the proprietor or sole trader who is identified as the business.</skos:definition>
      <rdfs:subPropertyOf rdf:resource="&fibo-be-fct-fct;functionalBusinessEntityTakesForm"/>
      <rdfs:domain rdf:resource="&fibo-be-fct-fct;SoleProprietorship"/>
      <rdfs:range rdf:resource="&fibo-be-le-lp;NaturalPerson"/>
   </owl:ObjectProperty>

   <owl:ObjectProperty rdf:about="&fibo-be-fct-fct;isCharacterizedBy">
      <rdfs:label>is characterized by</rdfs:label>
      <skos:definition>that context in which a contextually defined thing is defined</skos:definition>
      <rdfs:subPropertyOf rdf:resource="&fibo-uo-rl;inContext"/>
      <rdfs:domain rdf:resource="&fibo-fnd-rel-rel;Thing"/>
      <rdfs:range rdf:resource="&fibo-fnd-rel-rel;Thing"/>
   </owl:ObjectProperty>


  <!--
    ///////////////////////////////////////////////////////////////////////////////////////
    //
    // Data Properties
    //
    ///////////////////////////////////////////////////////////////////////////////////////
    -->



  <!--
    ///////////////////////////////////////////////////////////////////////////////////////
    //
    // Annotation Properties
    //
    ///////////////////////////////////////////////////////////////////////////////////////
    -->



  <!--
    ///////////////////////////////////////////////////////////////////////////////////////
    //
    // Classes
    //
    ///////////////////////////////////////////////////////////////////////////////////////
    -->


<owl:Class rdf:about="&fibo-be-fct-fct;BenefitCorporation">
      <rdfs:label>benefit corporation</rdfs:label>
      <skos:definition>Corporation set up under specific state legislation to provide some stated societal benefit, and with some corresponding relaxation of the obligation to maximize shareholder return.</skos:definition>
      <rdfs:subClassOf rdf:resource="&fibo-be-fct-fct;FunctionalBusinessEntity"/>
   </owl:Class>

   <owl:Class rdf:about="&fibo-be-fct-fct;Business">
      <rdfs:label>business</rdfs:label>
      <skos:definition>Some entity set up for the purposes of carrying out some commercial activities for profit.</skos:definition>
   </owl:Class>

   <owl:Class rdf:about="&fibo-be-fct-fct;Commerce">
      <rdfs:label>commerce</rdfs:label>
      <skos:definition>The activity of buying and selling goods.</skos:definition>
      <rdfs:subClassOf rdf:resource="&fibo-be-fct-fct;CommercialActivity"/>
   </owl:Class>

   <owl:Class rdf:about="&fibo-be-fct-fct;CommercialActivity">
      <rdfs:label>commercial activity</rdfs:label>
      <skos:definition>The context of carrying out trade and other comercial i.e. for-profit activities.</skos:definition>
      <rdfs:subClassOf rdf:resource="&fibo-rl-rbe;BusinessContext"/>
   </owl:Class>

   <owl:Class rdf:about="&fibo-be-fct-fct;CooperativeSociety">
      <rdfs:label>cooperative society</rdfs:label>
      <skos:definition>A commercial enterprise owned and managed by and for the benefit of customers or workers.</skos:definition>
   </owl:Class>

   <owl:Class rdf:about="&fibo-be-fct-fct;FamilyOffice">
      <rdfs:label>family office</rdfs:label>
      <skos:definition>Family Office as defined in the relevant legislation.</skos:definition>
   </owl:Class>

   <owl:Class rdf:about="&fibo-be-fct-fct;FunctionalBusinessEntity">
      <rdfs:label>functional business entity</rdfs:label>
      <skos:definition>A business entity defined in terms of its function.</skos:definition>
      <rdfs:subClassOf rdf:resource="&fibo-rl-rbe;RelativeBusinessEntity"/>
   </owl:Class>

   <owl:Class rdf:about="&fibo-be-fct-fct;Merchant">
      <rdfs:label>merchant</rdfs:label>
      <skos:definition>A business entity engaged in a trading activity. Fuether Notes: Defined in terms of its role.</skos:definition>
      <rdfs:subClassOf rdf:resource="&fibo-be-fct-fct;Business"/>
   </owl:Class>

   <owl:Class rdf:about="&fibo-be-fct-fct;NonProfitOrganization">
      <rdfs:label>non profit organization</rdfs:label>
      <skos:definition>An organization which exists for some purpose other than to make a profit for its participants.</skos:definition>
   </owl:Class>

   <owl:Class rdf:about="&fibo-be-fct-fct;SoleProprietorship">
      <rdfs:label>sole proprietorship</rdfs:label>
      <skos:definition>A business structure in which an individual and his/her company are considered a single entity for tax and liability purposes.</skos:definition>
   </owl:Class>


  <!--
    ///////////////////////////////////////////////////////////////////////////////////////
    //
    // Individuals
    //
    ///////////////////////////////////////////////////////////////////////////////////////
    -->


</rdf:RDF>