<?xml version="1.0" encoding="UTF-8"?>
<!DOCTYPE rdf:RDF [
	<!ENTITY dct "http://purl.org/dc/terms/">
	<!ENTITY fibo-be-le-fbo "https://spec.edmcouncil.org/fibo/ontology/BE/LegalEntities/FormalBusinessOrganizations/">
	<!ENTITY fibo-be-le-lp "https://spec.edmcouncil.org/fibo/ontology/BE/LegalEntities/LegalPersons/">
	<!ENTITY fibo-be-tr-tr "https://spec.edmcouncil.org/fibo/ontology/BE/Trusts/Trusts/">
	<!ENTITY fibo-fnd-agr-agr "https://spec.edmcouncil.org/fibo/ontology/FND/Agreements/Agreements/">
	<!ENTITY fibo-fnd-pty-pty "https://spec.edmcouncil.org/fibo/ontology/FND/Parties/Parties/">
	<!ENTITY fibo-fnd-pty-rl "https://spec.edmcouncil.org/fibo/ontology/FND/Parties/Roles/">
	<!ENTITY fibo-fnd-rel-rel "https://spec.edmcouncil.org/fibo/ontology/FND/Relations/Relations/">
	<!ENTITY fibo-fnd-utl-av "https://spec.edmcouncil.org/fibo/ontology/FND/Utilities/AnnotationVocabulary/">
	<!ENTITY lcc-lr "https://www.omg.org/spec/LCC/Languages/LanguageRepresentation/">
	<!ENTITY owl "http://www.w3.org/2002/07/owl#">
	<!ENTITY rdf "http://www.w3.org/1999/02/22-rdf-syntax-ns#">
	<!ENTITY rdfs "http://www.w3.org/2000/01/rdf-schema#">
	<!ENTITY skos "http://www.w3.org/2004/02/skos/core#">
	<!ENTITY sm "http://www.omg.org/techprocess/ab/SpecificationMetadata/">
	<!ENTITY xsd "http://www.w3.org/2001/XMLSchema#">
]>
<rdf:RDF xml:base="https://spec.edmcouncil.org/fibo/ontology/BE/Trusts/Trusts/"
	xmlns:dct="http://purl.org/dc/terms/"
	xmlns:fibo-be-le-fbo="https://spec.edmcouncil.org/fibo/ontology/BE/LegalEntities/FormalBusinessOrganizations/"
	xmlns:fibo-be-le-lp="https://spec.edmcouncil.org/fibo/ontology/BE/LegalEntities/LegalPersons/"
	xmlns:fibo-be-tr-tr="https://spec.edmcouncil.org/fibo/ontology/BE/Trusts/Trusts/"
	xmlns:fibo-fnd-agr-agr="https://spec.edmcouncil.org/fibo/ontology/FND/Agreements/Agreements/"
	xmlns:fibo-fnd-pty-pty="https://spec.edmcouncil.org/fibo/ontology/FND/Parties/Parties/"
	xmlns:fibo-fnd-pty-rl="https://spec.edmcouncil.org/fibo/ontology/FND/Parties/Roles/"
	xmlns:fibo-fnd-rel-rel="https://spec.edmcouncil.org/fibo/ontology/FND/Relations/Relations/"
	xmlns:fibo-fnd-utl-av="https://spec.edmcouncil.org/fibo/ontology/FND/Utilities/AnnotationVocabulary/"
	xmlns:lcc-lr="https://www.omg.org/spec/LCC/Languages/LanguageRepresentation/"
	xmlns:owl="http://www.w3.org/2002/07/owl#"
	xmlns:rdf="http://www.w3.org/1999/02/22-rdf-syntax-ns#"
	xmlns:rdfs="http://www.w3.org/2000/01/rdf-schema#"
	xmlns:skos="http://www.w3.org/2004/02/skos/core#"
	xmlns:sm="http://www.omg.org/techprocess/ab/SpecificationMetadata/"
	xmlns:xsd="http://www.w3.org/2001/XMLSchema#">
	
	<owl:Ontology rdf:about="https://spec.edmcouncil.org/fibo/ontology/BE/Trusts/Trusts/">
		<rdfs:label>Trusts Ontology</rdfs:label>
		<dct:abstract>This ontology defines the fundamental common terms for trusts. Trusts are entities set up in terms of the applicable local statutes goerning trusts, and have as a minimum three specific, defined parties, known in many jurisdictions as trustor (sometimes sponsor), trustee and beneficiary. The terms in this ontology may be extended as necessary to represent specific types of trust, for example in the funds arena.</dct:abstract>
		<dct:license rdf:datatype="&xsd;anyURI">http://opensource.org/licenses/MIT</dct:license>
		<sm:contentLanguage rdf:datatype="&xsd;anyURI">http://www.w3.org/standards/techs/owl#w3c_all</sm:contentLanguage>
		<sm:copyright>Copyright (c) 2013-2020 EDM Council, Inc.</sm:copyright>
		<sm:copyright>Copyright (c) 2013-2020 Object Management Group, Inc.</sm:copyright>
		<sm:dependsOn rdf:datatype="&xsd;anyURI">https://spec.edmcouncil.org/fibo/ontology/BE/LegalEntities/FormalBusinessOrganizations/</sm:dependsOn>
		<sm:dependsOn rdf:datatype="&xsd;anyURI">https://spec.edmcouncil.org/fibo/ontology/BE/LegalEntities/LegalPersons/</sm:dependsOn>
		<sm:dependsOn rdf:datatype="&xsd;anyURI">https://spec.edmcouncil.org/fibo/ontology/FND/</sm:dependsOn>
		<sm:dependsOn rdf:datatype="&xsd;anyURI">https://www.omg.org/spec/LCC/</sm:dependsOn>
		<sm:fileAbbreviation>fibo-be-tr-tr</sm:fileAbbreviation>
		<sm:filename>Trusts.rdf</sm:filename>
		<owl:imports rdf:resource="https://spec.edmcouncil.org/fibo/ontology/BE/LegalEntities/FormalBusinessOrganizations/"/>
		<owl:imports rdf:resource="https://spec.edmcouncil.org/fibo/ontology/BE/LegalEntities/LegalPersons/"/>
		<owl:imports rdf:resource="https://spec.edmcouncil.org/fibo/ontology/FND/Agreements/Agreements/"/>
		<owl:imports rdf:resource="https://spec.edmcouncil.org/fibo/ontology/FND/Parties/Parties/"/>
		<owl:imports rdf:resource="https://spec.edmcouncil.org/fibo/ontology/FND/Parties/Roles/"/>
		<owl:imports rdf:resource="https://spec.edmcouncil.org/fibo/ontology/FND/Relations/Relations/"/>
		<owl:imports rdf:resource="https://spec.edmcouncil.org/fibo/ontology/FND/Utilities/AnnotationVocabulary/"/>
		<owl:imports rdf:resource="https://www.omg.org/spec/LCC/Languages/LanguageRepresentation/"/>
		<owl:versionIRI rdf:resource="https://spec.edmcouncil.org/fibo/ontology/BE/20181101/Trusts/Trusts/"/>
		<skos:changeNote>The https://spec.edmcouncil.org/fibo/ontology/BE/20131101/Trusts/Trusts.rdf version of this ontology was modified per the issue resolutions identified in the FIBO BE 1.0 FTF report.</skos:changeNote>
		<skos:changeNote>The https://spec.edmcouncil.org/fibo/ontology/BE/20150201/Trusts/Trusts.rdf version of this ontology was modified per the FIBO 2.0 RFC.</skos:changeNote>
		<skos:changeNote>The https://spec.edmcouncil.org/fibo/ontology/BE/20180801/Trusts/Trusts.rdf version of this ontology was modified to simplify / merge the legal person and formal organization class hierarchies.</skos:changeNote>
		<skos:changeNote>The https://spec.edmcouncil.org/fibo/ontology/BE/20181101/Trusts/Trusts.rdf version of this ontology was modified to eliminate duplication with concepts in LCC.</skos:changeNote>
		<fibo-fnd-utl-av:hasMaturityLevel rdf:resource="&fibo-fnd-utl-av;Release"/>
	</owl:Ontology>
	
	<owl:Class rdf:about="&fibo-be-tr-tr;FundUnitHolder">
		<rdfs:subClassOf rdf:resource="&fibo-be-tr-tr;TrustBeneficiary"/>
		<rdfs:subClassOf>
			<owl:Restriction>
				<owl:onProperty rdf:resource="&fibo-fnd-rel-rel;hasIdentity"/>
				<owl:onClass rdf:resource="&fibo-be-le-lp;LegalPerson"/>
				<owl:qualifiedCardinality rdf:datatype="&xsd;nonNegativeInteger">1</owl:qualifiedCardinality>
			</owl:Restriction>
		</rdfs:subClassOf>
		<rdfs:subClassOf>
			<owl:Restriction>
				<owl:onProperty rdf:resource="&fibo-fnd-pty-rl;isPlayedBy"/>
				<owl:someValuesFrom>
					<owl:Restriction>
						<owl:onProperty rdf:resource="&fibo-fnd-pty-pty;isAPartyTo"/>
						<owl:onClass rdf:resource="&fibo-be-tr-tr;TrustFundTrust"/>
						<owl:qualifiedCardinality rdf:datatype="&xsd;nonNegativeInteger">1</owl:qualifiedCardinality>
					</owl:Restriction>
				</owl:someValuesFrom>
			</owl:Restriction>
		</rdfs:subClassOf>
		<rdfs:label>fund unit holder</rdfs:label>
		<skos:definition>a party that holds some unit in a fund</skos:definition>
	</owl:Class>
	
	<owl:Class rdf:about="&fibo-be-tr-tr;Trust">
		<rdfs:subClassOf rdf:resource="&fibo-be-le-lp;LegalEntity"/>
		<rdfs:subClassOf>
			<owl:Restriction>
				<owl:onProperty rdf:resource="&fibo-fnd-rel-rel;isGovernedBy"/>
				<owl:onClass rdf:resource="&fibo-be-tr-tr;TrustAgreement"/>
				<owl:qualifiedCardinality rdf:datatype="&xsd;nonNegativeInteger">1</owl:qualifiedCardinality>
			</owl:Restriction>
		</rdfs:subClassOf>
		<rdfs:subClassOf>
			<owl:Restriction>
				<owl:onProperty rdf:resource="&fibo-fnd-pty-pty;hasPartyInRole"/>
				<owl:someValuesFrom rdf:resource="&fibo-be-tr-tr;TrustBeneficiary"/>
			</owl:Restriction>
		</rdfs:subClassOf>
		<rdfs:subClassOf>
			<owl:Restriction>
				<owl:onProperty rdf:resource="&fibo-fnd-pty-pty;hasPartyInRole"/>
				<owl:someValuesFrom rdf:resource="&fibo-be-tr-tr;Trustee"/>
			</owl:Restriction>
		</rdfs:subClassOf>
		<rdfs:subClassOf>
			<owl:Restriction>
				<owl:onProperty rdf:resource="&fibo-fnd-pty-pty;hasPartyInRole"/>
				<owl:someValuesFrom rdf:resource="&fibo-be-tr-tr;Trustor"/>
			</owl:Restriction>
		</rdfs:subClassOf>
		<rdfs:label>trust</rdfs:label>
		<skos:definition>A fiduciary relationship in which one party, known as a trustor, gives another party, the trustee, the right to hold title to property or assets for the benefit of a third party, the beneficiary.</skos:definition>
		<skos:editorialNote>This is a legal agreement between parties that someone owns, and is thereby an asset that they own. They can be taxed on this as any other asset. There are generally accepted things such as the source of funds that will determine who the revenue agency will go after. Definition reference URL: http://www.investopedia.com/terms/t/trust.asp</skos:editorialNote>
	</owl:Class>
	
	<owl:Class rdf:about="&fibo-be-tr-tr;TrustAgreement">
		<rdfs:subClassOf rdf:resource="&fibo-be-le-fbo;OrganizationCoveringAgreement"/>
		<rdfs:subClassOf>
			<owl:Restriction>
				<owl:onProperty rdf:resource="&fibo-fnd-pty-pty;hasPartyInRole"/>
				<owl:someValuesFrom rdf:resource="&fibo-be-tr-tr;TrustBeneficiary"/>
			</owl:Restriction>
		</rdfs:subClassOf>
		<rdfs:subClassOf>
			<owl:Restriction>
				<owl:onProperty rdf:resource="&fibo-fnd-pty-pty;hasPartyInRole"/>
				<owl:someValuesFrom rdf:resource="&fibo-be-tr-tr;Trustee"/>
			</owl:Restriction>
		</rdfs:subClassOf>
		<rdfs:subClassOf>
			<owl:Restriction>
				<owl:onProperty rdf:resource="&fibo-fnd-pty-pty;hasPartyInRole"/>
				<owl:someValuesFrom rdf:resource="&fibo-be-tr-tr;Trustor"/>
			</owl:Restriction>
		</rdfs:subClassOf>
		<rdfs:label>trust agreement</rdfs:label>
		<skos:definition>Formal agreement through which a trustor vests the ownership rights (title) to one or more assets to one or more trustees for conservation and protection on behalf of one or more beneficiaries of the trust. It normally states the (1) purpose for which the trust was established and fulfillment of which will terminate the trust, (2) details of the assets placed in the trust, (3) powers and limitations of the trustees, their reporting requirements, and other associated provisions, and (4) may also specify the trustees&apos; compensation, if any. A trust agreement involving real estate requires its exact description and the trustor&apos;s express, written consent to create the trust to be valid. A will admitted to probate may also act like a trust agreement.</skos:definition>
		<skos:editorialNote>See also Deed. These are distinct from Contracts in that they impose obligations but without necessarily reciprocating rights.</skos:editorialNote>
		<fibo-fnd-utl-av:definitionOrigin rdf:datatype="&xsd;anyURI">http://www.businessdictionary.com/definition/trust-agreement.html</fibo-fnd-utl-av:definitionOrigin>
		<fibo-fnd-utl-av:synonym>trust deed</fibo-fnd-utl-av:synonym>
		<fibo-fnd-utl-av:synonym>trust document</fibo-fnd-utl-av:synonym>
		<fibo-fnd-utl-av:synonym>trust instrument</fibo-fnd-utl-av:synonym>
	</owl:Class>
	
	<owl:Class rdf:about="&fibo-be-tr-tr;TrustBeneficiary">
		<rdfs:subClassOf rdf:resource="&fibo-fnd-agr-agr;Beneficiary"/>
		<rdfs:subClassOf>
			<owl:Restriction>
				<owl:onProperty rdf:resource="&fibo-fnd-pty-rl;isPlayedBy"/>
				<owl:someValuesFrom>
					<owl:Restriction>
						<owl:onProperty rdf:resource="&fibo-fnd-pty-pty;isAPartyTo"/>
						<owl:allValuesFrom rdf:resource="&fibo-be-tr-tr;TrustAgreement"/>
					</owl:Restriction>
				</owl:someValuesFrom>
			</owl:Restriction>
		</rdfs:subClassOf>
		<rdfs:label>trust beneficiary</rdfs:label>
		<skos:definition>Person or organization for whose present or future interest (benefit) an annuity, assignment (such as a letter of credit), contract, insurance policy, judgment, promise, trust, will, etc., is made</skos:definition>
		<fibo-fnd-utl-av:definitionOrigin rdf:datatype="&xsd;anyURI">http://www.businessdictionary.com/definition/beneficiary.html</fibo-fnd-utl-av:definitionOrigin>
	</owl:Class>
	
	<owl:Class rdf:about="&fibo-be-tr-tr;TrustFundManager">
		<rdfs:subClassOf rdf:resource="&fibo-fnd-pty-pty;PartyInRole"/>
		<rdfs:subClassOf>
			<owl:Restriction>
				<owl:onProperty rdf:resource="&fibo-fnd-rel-rel;hasIdentity"/>
				<owl:allValuesFrom rdf:resource="&fibo-be-le-lp;LegalPerson"/>
			</owl:Restriction>
		</rdfs:subClassOf>
		<rdfs:subClassOf>
			<owl:Restriction>
				<owl:onProperty rdf:resource="&fibo-fnd-pty-rl;isPlayedBy"/>
				<owl:someValuesFrom>
					<owl:Restriction>
						<owl:onProperty rdf:resource="&fibo-fnd-rel-rel;manages"/>
						<owl:allValuesFrom rdf:resource="&fibo-be-tr-tr;Trust"/>
					</owl:Restriction>
				</owl:someValuesFrom>
			</owl:Restriction>
		</rdfs:subClassOf>
		<rdfs:label>trust fund manager</rdfs:label>
		<skos:definition>A trust fund manager acts on behalf of the Trustee to manage the assets of the Trust.</skos:definition>
	</owl:Class>
	
	<owl:Class rdf:about="&fibo-be-tr-tr;TrustFundTrust">
		<rdfs:subClassOf rdf:resource="&fibo-be-tr-tr;Trust"/>
		<rdfs:subClassOf>
			<owl:Restriction>
				<owl:onProperty rdf:resource="&fibo-fnd-rel-rel;isManagedBy"/>
				<owl:allValuesFrom rdf:resource="&fibo-be-tr-tr;TrustFundManager"/>
			</owl:Restriction>
		</rdfs:subClassOf>
		<rdfs:subClassOf>
			<owl:Restriction>
				<owl:onProperty rdf:resource="&fibo-fnd-pty-pty;hasPartyInRole"/>
				<owl:someValuesFrom rdf:resource="&fibo-be-tr-tr;FundUnitHolder"/>
			</owl:Restriction>
		</rdfs:subClassOf>
		<rdfs:label>trust fund trust</rdfs:label>
		<skos:definition>A trust which forms the basis for a fund.</skos:definition>
		<skos:editorialNote>The fund is identified as being a kind of Trust Fund.</skos:editorialNote>
	</owl:Class>
	
	<owl:Class rdf:about="&fibo-be-tr-tr;Trustee">
		<rdfs:subClassOf rdf:resource="&fibo-fnd-pty-pty;OrganizationMember"/>
		<rdfs:subClassOf>
			<owl:Restriction>
				<owl:onProperty rdf:resource="&fibo-fnd-rel-rel;hasIdentity"/>
				<owl:allValuesFrom rdf:resource="&fibo-be-le-lp;LegalPerson"/>
			</owl:Restriction>
		</rdfs:subClassOf>
		<rdfs:subClassOf>
			<owl:Restriction>
				<owl:onProperty rdf:resource="&fibo-fnd-pty-rl;isPlayedBy"/>
				<owl:someValuesFrom>
					<owl:Restriction>
						<owl:onProperty rdf:resource="&fibo-fnd-rel-rel;manages"/>
						<owl:allValuesFrom rdf:resource="&fibo-be-tr-tr;Trust"/>
					</owl:Restriction>
				</owl:someValuesFrom>
			</owl:Restriction>
		</rdfs:subClassOf>
		<rdfs:subClassOf>
			<owl:Restriction>
				<owl:onProperty rdf:resource="&fibo-fnd-pty-rl;isPlayedBy"/>
				<owl:someValuesFrom>
					<owl:Restriction>
						<owl:onProperty rdf:resource="&lcc-lr;isMemberOf"/>
						<owl:allValuesFrom rdf:resource="&fibo-be-tr-tr;Trust"/>
					</owl:Restriction>
				</owl:someValuesFrom>
			</owl:Restriction>
		</rdfs:subClassOf>
		<rdfs:subClassOf>
			<owl:Restriction>
				<owl:onProperty rdf:resource="&fibo-fnd-pty-rl;isPlayedBy"/>
				<owl:someValuesFrom>
					<owl:Restriction>
						<owl:onProperty rdf:resource="&fibo-fnd-pty-pty;isAPartyTo"/>
						<owl:onClass rdf:resource="&fibo-be-tr-tr;TrustAgreement"/>
						<owl:qualifiedCardinality rdf:datatype="&xsd;nonNegativeInteger">1</owl:qualifiedCardinality>
					</owl:Restriction>
				</owl:someValuesFrom>
			</owl:Restriction>
		</rdfs:subClassOf>
		<rdfs:label>trustee</rdfs:label>
		<skos:definition>An individual or organization which holds or manages and invests assets for the benefit of another. The trustee is legally obliged to make all trust-related decisions with the beneficiary&apos;s interests in mind, and may be liable for damages in the event of not doing so. Trustees may be entitled to a payment for their services, if specified in the trust deed. In the specific case of the bond market, a trustee administers a bond issue for a borrower, and ensures that the issuer meets all the terms and conditions associated with the borrowing.</skos:definition>
		<fibo-fnd-utl-av:definitionOrigin rdf:datatype="&xsd;anyURI">http://www.investorwords.com/5086/trustee.html</fibo-fnd-utl-av:definitionOrigin>
	</owl:Class>
	
	<owl:Class rdf:about="&fibo-be-tr-tr;Trustor">
		<rdfs:subClassOf rdf:resource="&fibo-fnd-pty-pty;OrganizationMember"/>
		<rdfs:subClassOf>
			<owl:Restriction>
				<owl:onProperty rdf:resource="&fibo-fnd-rel-rel;hasIdentity"/>
				<owl:allValuesFrom rdf:resource="&fibo-fnd-pty-pty;IndependentParty"/>
			</owl:Restriction>
		</rdfs:subClassOf>
		<rdfs:subClassOf>
			<owl:Restriction>
				<owl:onProperty rdf:resource="&fibo-fnd-pty-rl;isPlayedBy"/>
				<owl:someValuesFrom>
					<owl:Restriction>
						<owl:onProperty rdf:resource="&fibo-fnd-pty-pty;isAPartyTo"/>
						<owl:onClass rdf:resource="&fibo-be-tr-tr;TrustAgreement"/>
						<owl:qualifiedCardinality rdf:datatype="&xsd;nonNegativeInteger">1</owl:qualifiedCardinality>
					</owl:Restriction>
				</owl:someValuesFrom>
			</owl:Restriction>
		</rdfs:subClassOf>
		<rdfs:label>trustor</rdfs:label>
		<skos:definition>Entity that establishes a trust and place property under the protection and management of one or more trustees for the immediate or eventual benefit of ascertainable one or more beneficiaries. It is not always necessary to identify the trustor who may be also be a trustee and/or one of the beneficiaries. In legal parlance, a trustor is called a settlor in the UK and a grantor in the US, whereas in common usage he or she may also be called a creator, donor, initiator, owner, or Trust maker.</skos:definition>
		<fibo-fnd-utl-av:definitionOrigin rdf:datatype="&xsd;anyURI">http://www.businessdictionary.com/definition/trustor.html</fibo-fnd-utl-av:definitionOrigin>
		<fibo-fnd-utl-av:synonym>grantor</fibo-fnd-utl-av:synonym>
		<fibo-fnd-utl-av:synonym>settlor</fibo-fnd-utl-av:synonym>
	</owl:Class>

</rdf:RDF>