<?xml version="1.0" encoding="UTF-8"?>
<rdf:RDF xmlns:xsd="http://www.w3.org/2001/XMLSchema#"
         xmlns:sm="http://www.omg.org/techprocess/ab/SpecificationMetadata/"
         xmlns:fibo-fnd-utl-av="http://www.omg.org/spec/EDMC-FIBO/FND/Utilities/AnnotationVocabulary/"
         xmlns:rdf="http://www.w3.org/1999/02/22-rdf-syntax-ns#"
         xmlns:rdfs="http://www.w3.org/2000/01/rdf-schema#"
         xmlns:owl="http://www.w3.org/2002/07/owl#"
         xmlns:skos="http://www.w3.org/2004/02/skos/core#"
         xmlns:dc="http://purl.org/dc/terms/"
         xml:base="http://www.edmcouncil.org/spec/EDMC-SR/FND/Information/InfoCore/">

   <owl:Ontology rdf:about="http://www.edmcouncil.org/spec/EDMC-SR/FND/Information/InfoCore/">
      <owl:imports rdf:resource="http://www.edmcouncil.org/spec/EDMC-SR/UO/Lattice/"/>
   </owl:Ontology>

   <!--Datatypes-->

<!--Object Properties-->

<owl:ObjectProperty rdf:about="http://www.edmcouncil.org/spec/EDMC-SR/FND/Information/InfoCore/hasPart">
      <skos:definition>Some kind of written information (including possibly another document) which forms part of the document. Term origin:SR modeling</skos:definition>
      <rdfs:subPropertyOf rdf:resource="http://www.omg.org/spec/EDMC-SR/FND/Relations/Relations/hasPart"/>
      <rdfs:domain rdf:resource="http://www.edmcouncil.org/spec/EDMC-SR/FND/Information/InfoCore/Document"/>
      <rdfs:range rdf:resource="http://www.edmcouncil.org/spec/EDMC-SR/FND/Information/InfoCore/WrittenInformation"/>
   </owl:ObjectProperty>

   <owl:ObjectProperty rdf:about="http://www.edmcouncil.org/spec/EDMC-SR/FND/Information/InfoCore/informationFlow">
      <skos:definition>Information Flow, whereby one piece of information becomes another. The information which the information becomes. Term origin:SR modeling</skos:definition>
      <rdfs:domain rdf:resource="http://www.edmcouncil.org/spec/EDMC-SR/FND/Information/InfoCore/Information"/>
      <rdfs:range rdf:resource="http://www.edmcouncil.org/spec/EDMC-SR/FND/Information/InfoCore/Information"/>
   </owl:ObjectProperty>

   <owl:ObjectProperty rdf:about="http://www.edmcouncil.org/spec/EDMC-SR/FND/Information/InfoCore/derivedFrom">
      <skos:definition>What the information derives from or refers to in order to be complete.</skos:definition>
      <skos:editorialNote>This is semantically distinct from what the information is 'about'. Here, we refer to something (usually but not necessarily some other information) which is referred to in the course of arriving at this information. Examples include mathematical terms referred to in order to derive this information, which in turn is actually about something else (the 'is about' thing).</skos:editorialNote>
      <rdfs:domain rdf:resource="http://www.edmcouncil.org/spec/EDMC-SR/FND/Information/InfoCore/Information"/>
      <rdfs:range rdf:resource="http://www.w3.org/2002/07/owl#Thing"/>
   </owl:ObjectProperty>

   <owl:ObjectProperty rdf:about="http://www.edmcouncil.org/spec/EDMC-SR/FND/Information/InfoCore/details">
      <rdfs:domain rdf:resource="http://www.w3.org/2002/07/owl#Thing"/>
      <rdfs:range rdf:resource="http://www.edmcouncil.org/spec/EDMC-SR/FND/Information/InfoCore/Information"/>
      <owl:inverseOf rdf:resource="http://www.edmcouncil.org/spec/EDMC-SR/FND/Information/InfoCore/isAbout"/>
   </owl:ObjectProperty>

   <owl:ObjectProperty rdf:about="http://www.edmcouncil.org/spec/EDMC-SR/FND/Information/InfoCore/isAbout">
      <skos:definition>What the information is about</skos:definition>
      <rdfs:domain rdf:resource="http://www.edmcouncil.org/spec/EDMC-SR/FND/Information/InfoCore/Information"/>
      <rdfs:range rdf:resource="http://www.w3.org/2002/07/owl#Thing"/>
   </owl:ObjectProperty>

   <!--Data Properties-->

<owl:DatatypeProperty rdf:about="http://www.edmcouncil.org/spec/EDMC-SR/FND/Information/InfoCore/name">
      <rdfs:range rdf:resource="http://www.omg.org/spec/EDMC-SR/FND/Utilities/BusinessFacingTypes/text"/>
   </owl:DatatypeProperty>

   <!--Annotation Properties-->

<!--Classes-->

<owl:Class rdf:about="http://www.edmcouncil.org/spec/EDMC-SR/FND/Information/InfoCore/Document">
      <rdfs:label>Document</rdfs:label>
      <skos:definition>An information deliverable created in the course of some business process, and with some lifecycle independent of its use to communicate the information therein.</skos:definition>
      <skos:editorialNote>Documents are usually in sections and contain a multiplicity of information, generally on a given subject and for a given audience. In particular, documents generall have parts. This term is defined so that parts of documents may be defined. This is a difficult concept to define, but there is some value in distinguishing information of this sort, from memoranda, reports and the like. THis is particularly for the identification of things such as contracts, prospectuses and the like, as distinct from the elements of information which may make up their parts, and allowing for the possibility of these having different status at different times and so on (Draft document versus Formal Document). However, certain of those others (e.g. Report) may also be considered documents in some cases.</skos:editorialNote>
      <rdfs:subClassOf rdf:resource="http://www.edmcouncil.org/spec/EDMC-SR/FND/Information/InfoCore/WrittenInformation"/>
   </owl:Class>

   <owl:Class rdf:about="http://www.edmcouncil.org/spec/EDMC-SR/FND/Information/InfoCore/WrittenInformation">
      <rdfs:label>Written Information</rdfs:label>
      <skos:definition>Some information which is written in some format (physical or electronic) and is or may be communicated in some way.</skos:definition>
      <rdfs:subClassOf rdf:resource="http://www.edmcouncil.org/spec/EDMC-SR/UO/OntologicalDegree/IndependentThing"/>
      <rdfs:subClassOf rdf:resource="http://www.edmcouncil.org/spec/EDMC-SR/FND/Information/InfoCore/Information"/>
   </owl:Class>

   <owl:Class rdf:about="http://www.edmcouncil.org/spec/EDMC-SR/FND/Information/InfoCore/Information">
      <rdfs:label>Information</rdfs:label>
      <rdfs:subClassOf rdf:resource="http://www.edmcouncil.org/spec/EDMC-SR/UO/Lattice/Abstract"/>
   </owl:Class>

   <owl:Class rdf:about="http://www.edmcouncil.org/spec/EDMC-SR/FND/Information/InfoCore/Name">
      <rdfs:label>Name</rdfs:label>
      <rdfs:subClassOf rdf:resource="http://www.edmcouncil.org/spec/EDMC-SR/UO/Lattice/ContinuantThing"/>
   </owl:Class>

   <owl:Class rdf:about="http://www.edmcouncil.org/spec/EDMC-SR/FND/Information/InfoCore/StructuredName">
      <rdfs:label>Structured Name</rdfs:label>
      <skos:definition>A name with additional details besides simply being a string of text. This may include multilingual support or structuring of name content (as seen for example in financial securities names).</skos:definition>
      <rdfs:subClassOf rdf:resource="http://www.edmcouncil.org/spec/EDMC-SR/FND/Information/InfoCore/Name"/>
   </owl:Class>

   <!--Individuals-->

</rdf:RDF>