<?xml version="1.0" encoding="UTF-8"?>
<!DOCTYPE rdf:RDF [
	<!ENTITY dct "http://purl.org/dc/terms/">
	<!ENTITY fibo-be-le-fbo "https://spec.edmcouncil.org/fibo/BE/LegalEntities/FormalBusinessOrganizations/">
	<!ENTITY fibo-fnd-inf-doc "https://spec.edmcouncil.org/fibo/FND/InformationExt/Documentation/">
	<!ENTITY fibo-fnd-inf-inf "https://spec.edmcouncil.org/fibo/FND/InformationExt/InfoCore/">
	<!ENTITY fibo-fnd-pty-rl "https://spec.edmcouncil.org/fibo/FND/Parties/Roles/">
	<!ENTITY fibo-fnd-pub-pub "https://spec.edmcouncil.org/fibo/FND/PublicationsExt/Publications/">
	<!ENTITY fibo-fnd-rel-rel "https://spec.edmcouncil.org/fibo/FND/Relations/Relations/">
	<!ENTITY fibo-fnd-utl-av "https://spec.edmcouncil.org/fibo/FND/Utilities/AnnotationVocabulary/">
	<!ENTITY fibo-fnd-utl-val "https://spec.edmcouncil.org/fibo/FND/Utilities/Values/">
	<!ENTITY owl "http://www.w3.org/2002/07/owl#">
	<!ENTITY rdf "http://www.w3.org/1999/02/22-rdf-syntax-ns#">
	<!ENTITY rdfs "http://www.w3.org/2000/01/rdf-schema#">
	<!ENTITY skos "http://www.w3.org/2004/02/skos/core#">
	<!ENTITY xsd "http://www.w3.org/2001/XMLSchema#">
]>
<rdf:RDF
	xmlns:dct="http://purl.org/dc/terms/"
	xmlns:fibo-be-le-fbo="https://spec.edmcouncil.org/fibo/BE/LegalEntities/FormalBusinessOrganizations/"
	xmlns:fibo-fnd-inf-doc="https://spec.edmcouncil.org/fibo/FND/InformationExt/Documentation/"
	xmlns:fibo-fnd-inf-inf="https://spec.edmcouncil.org/fibo/FND/InformationExt/InfoCore/"
	xmlns:fibo-fnd-pty-rl="https://spec.edmcouncil.org/fibo/FND/Parties/Roles/"
	xmlns:fibo-fnd-pub-pub="https://spec.edmcouncil.org/fibo/FND/PublicationsExt/Publications/"
	xmlns:fibo-fnd-rel-rel="https://spec.edmcouncil.org/fibo/FND/Relations/Relations/"
	xmlns:fibo-fnd-utl-av="https://spec.edmcouncil.org/fibo/FND/Utilities/AnnotationVocabulary/"
	xmlns:fibo-fnd-utl-val="https://spec.edmcouncil.org/fibo/FND/Utilities/Values/"
	xmlns:owl="http://www.w3.org/2002/07/owl#"
	xmlns:rdf="http://www.w3.org/1999/02/22-rdf-syntax-ns#"
	xmlns:rdfs="http://www.w3.org/2000/01/rdf-schema#"
	xmlns:skos="http://www.w3.org/2004/02/skos/core#"
	xmlns:xsd="http://www.w3.org/2001/XMLSchema#">
	
	<owl:Ontology rdf:about="https://spec.edmcouncil.org/fibo/FND/PublicationsExt/Publications/">
		<rdfs:label xml:lang="en">Publications</rdfs:label>
		<dct:abstract>This ontology sets out the basic notions of published information and the entities that publish this. 
		Note that there is a convention in FIBO that, since the ontology is intended to be a computationally independent representation of real things in the world, no information construct (such as identifiers) is considered real unless it is published by someone. This ontology provides the conceptual underpinning for this notion and may not be needed in application ontologies.</dct:abstract>
		<owl:imports rdf:resource="http://www.w3.org/2004/02/skos/core"/>
		<owl:imports rdf:resource="https://spec.edmcouncil.org/fibo/BE/LegalEntities/FormalBusinessOrganizations/"/>
		<owl:imports rdf:resource="https://spec.edmcouncil.org/fibo/FND/InformationExt/Documentation/"/>
		<owl:imports rdf:resource="https://spec.edmcouncil.org/fibo/FND/InformationExt/InfoCore/"/>
		<owl:imports rdf:resource="https://spec.edmcouncil.org/fibo/FND/MathExt/Math/"/>
		<owl:imports rdf:resource="https://spec.edmcouncil.org/fibo/FND/Parties/Roles/"/>
		<owl:imports rdf:resource="https://spec.edmcouncil.org/fibo/FND/Relations/Relations/"/>
		<owl:imports rdf:resource="https://spec.edmcouncil.org/fibo/FND/Utilities/AnnotationVocabulary/"/>
		<owl:imports rdf:resource="https://spec.edmcouncil.org/fibo/FND/Utilities/Values/"/>
		<owl:versionIRI rdf:resource="https://spec.edmcouncil.org/fibo/FND/PublicationsExt/Publications/"/>
		<fibo-fnd-utl-av:hasMaturityLevel rdf:resource="&fibo-fnd-utl-av;Informative"/>
	</owl:Ontology>
	
	<owl:Class rdf:about="&fibo-fnd-pub-pub;PublishedInformation">
		<rdfs:subClassOf rdf:resource="&fibo-fnd-inf-inf;Information"/>
		<rdfs:subClassOf>
			<owl:Restriction>
				<owl:onProperty rdf:resource="&fibo-fnd-inf-inf;isAbout"/>
				<owl:someValuesFrom rdf:resource="&owl;Thing"/>
			</owl:Restriction>
		</rdfs:subClassOf>
		<rdfs:subClassOf>
			<owl:Restriction>
				<owl:onProperty rdf:resource="&fibo-fnd-pub-pub;publishedBy"/>
				<owl:someValuesFrom rdf:resource="&fibo-fnd-pub-pub;Publisher"/>
			</owl:Restriction>
		</rdfs:subClassOf>
		<rdfs:label xml:lang="en">published information</rdfs:label>
		<skos:definition xml:lang="en">Information put into the public domain by some party or sold at a profit.</skos:definition>
	</owl:Class>
	
	<owl:Class rdf:about="&fibo-fnd-pub-pub;Publisher">
		<rdfs:subClassOf rdf:resource="&fibo-fnd-pty-rl;AgentInRole"/>
		<rdfs:subClassOf>
			<owl:Restriction>
				<owl:onProperty rdf:resource="&fibo-fnd-pub-pub;publisherIdentity"/>
				<owl:someValuesFrom rdf:resource="&fibo-be-le-fbo;FormallyConstitutedOrganization"/>
			</owl:Restriction>
		</rdfs:subClassOf>
		<rdfs:label xml:lang="en">publisher</rdfs:label>
		<skos:definition xml:lang="en">An organization (such as a publishing house) which makes information. available.</skos:definition>
		<fibo-fnd-utl-av:explanatoryNote xml:lang="en">This is the role of publisher, whether or not the role is filled by a publishing house. For example it may also be the entity which publishes standard contract terms, e.g. an industry association or an exchange.</fibo-fnd-utl-av:explanatoryNote>
	</owl:Class>
	
	<owl:Class rdf:about="&fibo-fnd-pub-pub;PublishingHouse">
		<rdfs:subClassOf rdf:resource="&fibo-be-le-fbo;FormallyConstitutedOrganization"/>
		<rdfs:label xml:lang="en">publishing house</rdfs:label>
		<skos:definition xml:lang="en">Some business entity which specializes in publishing information.</skos:definition>
	</owl:Class>
	
	<owl:Class rdf:about="&fibo-fnd-pub-pub;WebPage">
		<rdfs:subClassOf rdf:resource="&fibo-fnd-inf-doc;Document"/>
		<rdfs:label xml:lang="en">web page</rdfs:label>
		<skos:definition xml:lang="en">A document published on the World Wide Web and accessible via a Universal Resource Locator.</skos:definition>
	</owl:Class>
	
	<owl:DatatypeProperty rdf:about="&fibo-fnd-pub-pub;brandName">
		<rdfs:label xml:lang="en">brand name</rdfs:label>
		<rdfs:domain rdf:resource="&fibo-fnd-pub-pub;Publisher"/>
		<rdfs:range rdf:resource="&xsd;string"/>
		<skos:definition xml:lang="en">The name of marque by which the publisher is identified in its publications. This may or may not be identical to the legal name or the Trading As name, but represents a separate semantic. Usually to be found on book jackets, press releases etc.</skos:definition>
	</owl:DatatypeProperty>
	
	<owl:ObjectProperty rdf:about="&fibo-fnd-pub-pub;publishedBy">
		<rdfs:subPropertyOf rdf:resource="&fibo-fnd-rel-rel;isProvidedBy"/>
		<rdfs:label xml:lang="en">is published by</rdfs:label>
		<rdfs:domain rdf:resource="&fibo-fnd-pub-pub;PublishedInformation"/>
		<rdfs:range rdf:resource="&fibo-fnd-pub-pub;Publisher"/>
		<skos:definition xml:lang="en">The organization which makes this information available.</skos:definition>
	</owl:ObjectProperty>
	
	<owl:ObjectProperty rdf:about="&fibo-fnd-pub-pub;publisherIdentity">
		<rdfs:subPropertyOf rdf:resource="&fibo-fnd-rel-rel;hasIdentity"/>
		<rdfs:label xml:lang="en">publisher identity</rdfs:label>
		<rdfs:domain rdf:resource="&fibo-fnd-pub-pub;Publisher"/>
		<rdfs:range rdf:resource="&fibo-be-le-fbo;FormallyConstitutedOrganization"/>
		<skos:definition xml:lang="en">A publisher of information may be identified as any Business Entity, including for example specialized publishing house, ratings agency, standards body and so on.</skos:definition>
	</owl:ObjectProperty>
	
	<owl:ObjectProperty rdf:about="&fibo-fnd-pub-pub;publishes">
		<rdfs:subPropertyOf rdf:resource="&fibo-fnd-rel-rel;provides"/>
		<rdfs:label xml:lang="en">publishes</rdfs:label>
		<rdfs:domain rdf:resource="&fibo-fnd-pub-pub;Publisher"/>
		<rdfs:range rdf:resource="&fibo-fnd-pub-pub;PublishedInformation"/>
	</owl:ObjectProperty>
	
	<owl:ObjectProperty rdf:about="&fibo-fnd-pub-pub;uRL">
		<rdfs:label xml:lang="en">u r l</rdfs:label>
		<rdfs:domain rdf:resource="&fibo-fnd-pub-pub;WebPage"/>
		<rdfs:range rdf:resource="&fibo-fnd-utl-val;URIValue"/>
		<skos:definition xml:lang="en">The URL of the web page.</skos:definition>
	</owl:ObjectProperty>

</rdf:RDF>