<?xml version="1.0" encoding="UTF-8"?>
  
<!DOCTYPE rdf:RDF [
    <!ENTITY fibo-fnd-agrx-ele "http://spec.edmcouncil.org/fibo/red/fnd/agreements-ext/contract-elements/">
    <!ENTITY fibo-rl-mer "http://spec.edmcouncil.org/fibo/red/fnd/relative/mereological/">
    <!ENTITY fibo-fnd-info-info "http://spec.edmcouncil.org/fibo/red/fnd/information/info-core/">
    <!ENTITY fibo-fnd-info-idn "http://spec.edmcouncil.org/fibo/red/fnd/information/identification/">
    <!ENTITY fibo-be-le-lei "http://spec.edmcouncil.org/fibo/red/be/legal-entities/lei-entities/">
    <!ENTITY fibo-fnd-agrx-ext "http://spec.edmcouncil.org/fibo/red/fnd/agreements-ext/contracts-extensions/">
    <!ENTITY fibo-be-le-fbo "http://spec.edmcouncil.org/fibo/red/be/legal-entities/formal-business-organizations/">
    <!ENTITY fibo-fnd-agr-ctr "http://spec.edmcouncil.org/fibo/red/fnd/agreements/contracts/">
]>

<rdf:RDF xmlns:xsd="http://www.w3.org/2001/XMLSchema#"
         xmlns:sm="http://www.omg.org/techprocess/ab/SpecificationMetadata/"
         xmlns:xs="http://www.w3.org/2001/XMLSchema"
         xmlns:fibo-fnd-utl-av="http://www.omg.org/spec/EDMC-FIBO/FND/Utilities/AnnotationVocabulary/"
         xmlns:rdf="http://www.w3.org/1999/02/22-rdf-syntax-ns#"
         xmlns:rdfs="http://www.w3.org/2000/01/rdf-schema#"
         xmlns:owl="http://www.w3.org/2002/07/owl#"
         xmlns:skos="http://www.w3.org/2004/02/skos/core#"
         xmlns:dc="http://purl.org/dc/terms/"
         xml:base="http://spec.edmcouncil.org/fibo/red/fnd/agreements-ext/contract-elements/">

   <owl:Ontology rdf:about="http://spec.edmcouncil.org/fibo/red/fnd/agreements-ext/contract-elements/">
      <owl:imports rdf:resource="http://spec.edmcouncil.org/fibo/red/fnd/relative/mereological/"/>
      <owl:imports rdf:resource="http://spec.edmcouncil.org/fibo/red/fnd/information/info-core/"/>
      <owl:imports rdf:resource="http://spec.edmcouncil.org/fibo/red/fnd/information/identification/"/>
      <owl:imports rdf:resource="http://spec.edmcouncil.org/fibo/red/be/legal-entities/lei-entities/"/>
      <owl:imports rdf:resource="http://spec.edmcouncil.org/fibo/red/fnd/agreements-ext/contracts-extensions/"/>
      <owl:imports rdf:resource="http://spec.edmcouncil.org/fibo/red/be/legal-entities/formal-business-organizations/"/>
      <owl:imports rdf:resource="http://spec.edmcouncil.org/fibo/red/fnd/agreements/contracts/"/>
   </owl:Ontology>


  <!--
    ///////////////////////////////////////////////////////////////////////////////////////
    //
    // Datatypes
    //
    ///////////////////////////////////////////////////////////////////////////////////////
    -->



  <!--
    ///////////////////////////////////////////////////////////////////////////////////////
    //
    // Object Properties
    //
    ///////////////////////////////////////////////////////////////////////////////////////
    -->


<owl:ObjectProperty rdf:about="&fibo-fnd-agrx-ele;IdentifiesContractPartyAs">
      <rdfs:label>identifies contract party as</rdfs:label>
      <skos:definition>The business entities identified in the contact party identification.</skos:definition>
      <rdfs:domain rdf:resource="&fibo-fnd-agrx-ele;ContractPartyIdentification"/>
      <rdfs:range rdf:resource="&fibo-be-le-lei;ContractuallyCapableEntity"/>
   </owl:ObjectProperty>

   <owl:ObjectProperty rdf:about="&fibo-fnd-agrx-ele;clauseContainsTerm">
      <rdfs:label>clause contains term</rdfs:label>
      <skos:definition>An individual term contained within the clause.</skos:definition>
      <rdfs:subPropertyOf rdf:resource="&fibo-fnd-agrx-ele;writtenContractHasPart"/>
      <rdfs:domain rdf:resource="&fibo-fnd-agrx-ele;ContractClause"/>
      <rdfs:range rdf:resource="&fibo-fnd-agrx-ele;ContractTerm"/>
   </owl:ObjectProperty>

   <owl:ObjectProperty rdf:about="&fibo-fnd-agrx-ele;identifies">
      <rdfs:label>identifies</rdfs:label>
      <skos:definition>A party identified in the contract party identification.</skos:definition>
      <rdfs:subPropertyOf rdf:resource="&fibo-fnd-info-idn;identifies"/>
      <rdfs:domain rdf:resource="&fibo-fnd-agrx-ele;ContractPartyIdentification"/>
      <rdfs:range rdf:resource="&fibo-fnd-agrx-ext;ContractParty"/>
   </owl:ObjectProperty>

   <owl:ObjectProperty rdf:about="&fibo-fnd-agrx-ele;definesPrincipals">
      <rdfs:label>defines principals</rdfs:label>
      <skos:definition>The identification of parties to the contract as embodied in the preamble.</skos:definition>
      <rdfs:domain rdf:resource="&fibo-fnd-agrx-ele;ContractPreamble"/>
      <rdfs:range rdf:resource="&fibo-fnd-agrx-ele;ContractPrincipalsIdentification"/>
   </owl:ObjectProperty>

   <owl:ObjectProperty rdf:about="&fibo-fnd-agrx-ele;identifiesPrincipal">
      <rdfs:label>identifies principal</rdfs:label>
      <skos:definition>The principal to the contract, identified in the contract principals identification.</skos:definition>
      <rdfs:subPropertyOf rdf:resource="&fibo-fnd-agrx-ele;identifies"/>
      <rdfs:domain rdf:resource="&fibo-fnd-agrx-ele;ContractPrincipalsIdentification"/>
      <rdfs:range rdf:resource="&fibo-fnd-agr-ctr;ContractPrincipal"/>
   </owl:ObjectProperty>

   <owl:ObjectProperty rdf:about="&fibo-fnd-agrx-ele;identifiesCounterparty">
      <rdfs:label>identifies counterparty</rdfs:label>
      <skos:definition>The counterparty to the contract, identified in the contract principals identification.</skos:definition>
      <rdfs:subPropertyOf rdf:resource="&fibo-fnd-agrx-ele;identifies"/>
      <rdfs:domain rdf:resource="&fibo-fnd-agrx-ele;ContractPrincipalsIdentification"/>
      <rdfs:range rdf:resource="&fibo-fnd-agr-ctr;ContractCounterparty"/>
   </owl:ObjectProperty>

   <owl:ObjectProperty rdf:about="&fibo-fnd-agrx-ele;hasTerm">
      <rdfs:label>has term</rdfs:label>
      <skos:definition>An individual term within the contractual terms set.</skos:definition>
      <rdfs:domain rdf:resource="&fibo-fnd-agr-ctr;ContractTermsSet"/>
      <rdfs:range rdf:resource="&fibo-fnd-agrx-ele;ContractTerm"/>
   </owl:ObjectProperty>

   <owl:ObjectProperty rdf:about="&fibo-fnd-agrx-ele;identifiesThirdParty">
      <rdfs:label>identifies third party</rdfs:label>
      <skos:definition>A third party identified in the third party identification.</skos:definition>
      <rdfs:subPropertyOf rdf:resource="&fibo-fnd-agrx-ele;identifies"/>
      <rdfs:domain rdf:resource="&fibo-fnd-agrx-ele;ContractThirdPartyIdentification"/>
      <rdfs:range rdf:resource="&fibo-fnd-agr-ctr;ContractThirdParty"/>
   </owl:ObjectProperty>

   <owl:ObjectProperty rdf:about="&fibo-fnd-agrx-ele;identifiesAs">
      <rdfs:label>identifies as</rdfs:label>
      <skos:definition>The business entity which is identified as a third party.</skos:definition>
      <rdfs:subPropertyOf rdf:resource="&fibo-fnd-agrx-ele;IdentifiesContractPartyAs"/>
      <rdfs:domain rdf:resource="&fibo-fnd-agrx-ele;ContractThirdPartyIdentification"/>
      <rdfs:range rdf:resource="&fibo-be-le-fbo;FormallyConstitutedOrganization"/>
   </owl:ObjectProperty>

   <owl:ObjectProperty rdf:about="&fibo-fnd-agrx-ele;principalsIdentification">
      <rdfs:label>principals identification</rdfs:label>
      <skos:definition>The identification of the principals of the contract.</skos:definition>
      <rdfs:domain rdf:resource="&fibo-fnd-agr-ctr;Contract"/>
      <rdfs:range rdf:resource="&fibo-fnd-agrx-ele;ContractPartyIdentification"/>
   </owl:ObjectProperty>

   <owl:ObjectProperty rdf:about="&fibo-fnd-agrx-ele;sectionContainsClause">
      <rdfs:label>section contains clause</rdfs:label>
      <skos:definition>A clause contained in the contract section.</skos:definition>
      <rdfs:subPropertyOf rdf:resource="&fibo-fnd-agrx-ele;writtenContractHasPart"/>
      <rdfs:domain rdf:resource="&fibo-fnd-agrx-ele;ContractSection"/>
      <rdfs:range rdf:resource="&fibo-fnd-agrx-ele;ContractClause"/>
   </owl:ObjectProperty>

   <owl:ObjectProperty rdf:about="&fibo-fnd-agrx-ele;defines">
      <rdfs:label>defines</rdfs:label>
      <skos:definition>The definition of some matter as agreed by the parties to the contract and written in some part of that contract.</skos:definition>
      <rdfs:domain rdf:resource="&fibo-fnd-agr-ctr;WrittenContract"/>
      <rdfs:range rdf:resource="&fibo-fnd-agr-ctr;ContractualDefinition"/>
   </owl:ObjectProperty>

   <owl:ObjectProperty rdf:about="&fibo-fnd-agrx-ele;definedInClause">
      <rdfs:label>defined in clause</rdfs:label>
      <skos:definition>The individual clause of the contract in which the set of terms is defined, if applicable.</skos:definition>
      <rdfs:subPropertyOf rdf:resource="&fibo-fnd-agrx-ele;definedInSection"/>
      <rdfs:domain rdf:resource="&fibo-fnd-agr-ctr;ContractTermsSet"/>
      <rdfs:range rdf:resource="&fibo-fnd-agrx-ele;ContractClause"/>
   </owl:ObjectProperty>

   <owl:ObjectProperty rdf:about="&fibo-fnd-agrx-ele;definedInSection">
      <rdfs:label>defined in section</rdfs:label>
      <skos:definition>The section of the contract in which the contract terms set is defined.</skos:definition>
      <rdfs:domain rdf:resource="&fibo-fnd-agr-ctr;ContractTermsSet"/>
      <rdfs:range rdf:resource="&fibo-fnd-agrx-ele;ContractSection"/>
   </owl:ObjectProperty>

   <owl:ObjectProperty rdf:about="&fibo-fnd-agrx-ele;identifiesContractPrincipalAs">
      <rdfs:label>identifies contract principal as</rdfs:label>
      <skos:definition>The business entities which are identified as the principals to the contract.</skos:definition>
      <rdfs:subPropertyOf rdf:resource="&fibo-fnd-agrx-ele;IdentifiesContractPartyAs"/>
      <rdfs:domain rdf:resource="&fibo-fnd-agrx-ele;ContractPrincipalsIdentification"/>
      <rdfs:range rdf:resource="&fibo-be-le-lei;ContractuallyCapableEntity"/>
   </owl:ObjectProperty>

   <owl:ObjectProperty rdf:about="&fibo-fnd-agrx-ele;writtenContractHasPart">
      <rdfs:label>written contract has part</rdfs:label>
      <skos:definition>A formal part of the contract such as a clause or term.</skos:definition>
      <rdfs:subPropertyOf rdf:resource="&fibo-fnd-info-info;hasPart"/>
      <rdfs:domain rdf:resource="&fibo-fnd-agr-ctr;WrittenContract"/>
      <rdfs:range rdf:resource="&fibo-fnd-agrx-ele;ContractPart"/>
   </owl:ObjectProperty>


  <!--
    ///////////////////////////////////////////////////////////////////////////////////////
    //
    // Data Properties
    //
    ///////////////////////////////////////////////////////////////////////////////////////
    -->



  <!--
    ///////////////////////////////////////////////////////////////////////////////////////
    //
    // Annotation Properties
    //
    ///////////////////////////////////////////////////////////////////////////////////////
    -->



  <!--
    ///////////////////////////////////////////////////////////////////////////////////////
    //
    // Classes
    //
    ///////////////////////////////////////////////////////////////////////////////////////
    -->


<owl:Class rdf:about="&fibo-fnd-agrx-ele;ContractClause">
      <rdfs:label>contract clause</rdfs:label>
      <skos:definition>A set of contractual terms, grouped according to subject, intent or the type of rights and / or obligations to which it refers.</skos:definition>
      <rdfs:subClassOf rdf:resource="&fibo-fnd-agrx-ele;ContractPart"/>
   </owl:Class>

   <owl:Class rdf:about="&fibo-fnd-agrx-ele;ContractPart">
      <rdfs:label>contract part</rdfs:label>
      <skos:definition>A formal part of a contract such as a clause or term.</skos:definition>
      <rdfs:subClassOf rdf:resource="&fibo-fnd-agr-ctr;ContractualElement"/>
      <rdfs:subClassOf rdf:resource="&fibo-fnd-info-info;WrittenInformation"/>
      <rdfs:subClassOf rdf:resource="&fibo-rl-mer;Part"/>
   </owl:Class>

   <owl:Class rdf:about="&fibo-fnd-agrx-ele;ContractPartyIdentification">
      <rdfs:label>contract party identification</rdfs:label>
      <skos:definition>The identification of parties to a contract. This is usually but not necessarily identified in the preamble to a contract.</skos:definition>
      <rdfs:subClassOf rdf:resource="&fibo-fnd-info-idn;PartyIdentification"/>
   </owl:Class>

   <owl:Class rdf:about="&fibo-fnd-agrx-ele;ContractPreamble">
      <rdfs:label>contract preamble</rdfs:label>
      <skos:definition>The part of a contract which defines the parties and gives sufficient information for them to be unambiguously identified, along with other pertinent information such as the subject of the contract.</skos:definition>
   </owl:Class>

   <owl:Class rdf:about="&fibo-fnd-agrx-ele;ContractPrincipalsIdentification">
      <rdfs:label>contract principals identification</rdfs:label>
      <skos:definition>The identification of the principals to a contract.</skos:definition>
      <rdfs:subClassOf rdf:resource="&fibo-fnd-agrx-ele;ContractPartyIdentification"/>
   </owl:Class>

   <owl:Class rdf:about="&fibo-fnd-agrx-ele;ContractSection">
      <rdfs:label>contract section</rdfs:label>
      <skos:definition>A formally identified Section of a Contract, comtaining terms dealing with a specific type of subject matter.</skos:definition>
   </owl:Class>

   <owl:Class rdf:about="&fibo-fnd-agrx-ele;ContractTerm">
      <rdfs:label>contract term</rdfs:label>
      <skos:definition>An individual term in a Contract. Forms part of a set of Contractual Terms. Also exists within a Clause of a Contract A Clause exists within a Section of a Contract</skos:definition>
   </owl:Class>

   <owl:Class rdf:about="&fibo-fnd-agrx-ele;ContractThirdPartyIdentification">
      <rdfs:label>contract third party identification</rdfs:label>
      <skos:definition>The identification of any third parties referred to in a contract but not being signatories to that contract. This would for example be the identification of calculation agents in a derivatives contract.</skos:definition>
   </owl:Class>

   <owl:Class rdf:about="&fibo-fnd-agrx-ele;RepresentationsSection">
      <rdfs:label>representations section</rdfs:label>
      <skos:definition>Section containing statements held out by one party to the other as being true and correct at the time of the Agreement. A representation, as contained in this section of a contract, is a statement by one other party asserting that some given state of the world exists.</skos:definition>
   </owl:Class>

   <owl:Class rdf:about="&fibo-fnd-agrx-ele;WarrantiesSection">
      <rdfs:label>warranties section</rdfs:label>
      <skos:definition>Section defining what is warranted by either party to the other. A warranty, as contained in this section of a contract, is a statement by one other party asserting that some given state of the world exists.</skos:definition>
   </owl:Class>

   <owl:Class rdf:about="&fibo-fnd-agrx-ele;DRIP">
      <rdfs:label>d r i p</rdfs:label>
      <skos:definition>A kind of financial contract.</skos:definition>
      <rdfs:subClassOf rdf:resource="&fibo-fnd-agr-ctr;BilateralContract"/>
   </owl:Class>


  <!--
    ///////////////////////////////////////////////////////////////////////////////////////
    //
    // Individuals
    //
    ///////////////////////////////////////////////////////////////////////////////////////
    -->


</rdf:RDF>