<?xml version="1.0" encoding="UTF-8"?>
  
<!DOCTYPE rdf:RDF [
    <!ENTITY fibo-fnd-info-info "http://spec.edmcouncil.org/fibo/red/fnd/information/info-core/">
    <!ENTITY fibo-uo-lat "http://spec.edmcouncil.org/fibo/red/uo/lattice/">
    <!ENTITY fibo-fnd-rel-rel "http://spec.edmcouncil.org/fibo/red/fnd/relations/relations/">
    <!ENTITY fibo-fnd-utl-bt "http://spec.edmcouncil.org/fibo/red/fnd/utilities/business-facing-types/">
    <!ENTITY fibo-uo-rl "http://spec.edmcouncil.org/fibo/red/uo/relatives/">
]>

<rdf:RDF xmlns:xsd="http://www.w3.org/2001/XMLSchema#"
         xmlns:sm="http://www.omg.org/techprocess/ab/SpecificationMetadata/"
         xmlns:xs="http://www.w3.org/2001/XMLSchema"
         xmlns:fibo-fnd-utl-av="http://www.omg.org/spec/EDMC-FIBO/FND/Utilities/AnnotationVocabulary/"
         xmlns:rdf="http://www.w3.org/1999/02/22-rdf-syntax-ns#"
         xmlns:rdfs="http://www.w3.org/2000/01/rdf-schema#"
         xmlns:owl="http://www.w3.org/2002/07/owl#"
         xmlns:skos="http://www.w3.org/2004/02/skos/core#"
         xmlns:dc="http://purl.org/dc/terms/"
         xml:base="http://spec.edmcouncil.org/fibo/red/fnd/information/info-core/">

   <owl:Ontology rdf:about="http://spec.edmcouncil.org/fibo/red/fnd/information/info-core/">
      <owl:imports rdf:resource="http://spec.edmcouncil.org/fibo/red/uo/lattice/"/>
      <owl:imports rdf:resource="http://spec.edmcouncil.org/fibo/red/fnd/relations/relations/"/>
      <owl:imports rdf:resource="http://spec.edmcouncil.org/fibo/red/fnd/utilities/business-facing-types/"/>
      <owl:imports rdf:resource="http://spec.edmcouncil.org/fibo/red/uo/relatives/"/>
   </owl:Ontology>


  <!--
    ///////////////////////////////////////////////////////////////////////////////////////
    //
    // Datatypes
    //
    ///////////////////////////////////////////////////////////////////////////////////////
    -->



  <!--
    ///////////////////////////////////////////////////////////////////////////////////////
    //
    // Object Properties
    //
    ///////////////////////////////////////////////////////////////////////////////////////
    -->


<owl:ObjectProperty rdf:about="&fibo-fnd-info-info;hasPart">
      <rdfs:label>has part</rdfs:label>
      <skos:definition>Some kind of written information (including possibly another document) which forms part of the document. Term origin:SR modeling</skos:definition>
      <rdfs:subPropertyOf rdf:resource="&fibo-fnd-rel-rel;hasPart"/>
      <rdfs:domain rdf:resource="&fibo-fnd-info-info;Document"/>
      <rdfs:range rdf:resource="&fibo-fnd-info-info;WrittenInformation"/>
   </owl:ObjectProperty>

   <owl:ObjectProperty rdf:about="&fibo-fnd-info-info;informationFlow">
      <rdfs:label>information flow</rdfs:label>
      <skos:definition>Information Flow, whereby one piece of information becomes another. The information which the information becomes. Term origin:SR modeling</skos:definition>
      <rdfs:domain rdf:resource="&fibo-fnd-info-info;Information"/>
      <rdfs:range rdf:resource="&fibo-fnd-info-info;Information"/>
   </owl:ObjectProperty>

   <owl:ObjectProperty rdf:about="&fibo-fnd-info-info;derivedFrom">
      <rdfs:label>derived from</rdfs:label>
      <skos:definition>What the information derives from or refers to in order to be complete.</skos:definition>
      <rdfs:domain rdf:resource="&fibo-fnd-info-info;Information"/>
      <rdfs:range rdf:resource="http://www.w3.org/2002/07/owl#Thing"/>
   </owl:ObjectProperty>

   <owl:ObjectProperty rdf:about="&fibo-fnd-info-info;details">
      <rdfs:label>details</rdfs:label>
      <rdfs:domain rdf:resource="http://www.w3.org/2002/07/owl#Thing"/>
      <rdfs:range rdf:resource="&fibo-fnd-info-info;Information"/>
      <owl:inverseOf rdf:resource="&fibo-fnd-info-info;isAbout"/>
   </owl:ObjectProperty>

   <owl:ObjectProperty rdf:about="&fibo-fnd-info-info;isAbout">
      <rdfs:label>is about</rdfs:label>
      <skos:definition>What the information is about</skos:definition>
      <rdfs:domain rdf:resource="&fibo-fnd-info-info;Information"/>
      <rdfs:range rdf:resource="http://www.w3.org/2002/07/owl#Thing"/>
   </owl:ObjectProperty>


  <!--
    ///////////////////////////////////////////////////////////////////////////////////////
    //
    // Data Properties
    //
    ///////////////////////////////////////////////////////////////////////////////////////
    -->


<owl:DatatypeProperty rdf:about="&fibo-fnd-info-info;name">
      <rdfs:label>name</rdfs:label>
      <skos:definition>The textual string which forms the name. In the case of a human being, this primary name becomes the surname.</skos:definition>
      <rdfs:range rdf:resource="&fibo-fnd-utl-bt;text"/>
   </owl:DatatypeProperty>


  <!--
    ///////////////////////////////////////////////////////////////////////////////////////
    //
    // Annotation Properties
    //
    ///////////////////////////////////////////////////////////////////////////////////////
    -->



  <!--
    ///////////////////////////////////////////////////////////////////////////////////////
    //
    // Classes
    //
    ///////////////////////////////////////////////////////////////////////////////////////
    -->


<owl:Class rdf:about="&fibo-fnd-info-info;Document">
      <rdfs:label>document</rdfs:label>
      <skos:definition>An information deliverable created in the course of some business process, and with some lifecycle independent of its use to communicate the information therein.</skos:definition>
      <rdfs:subClassOf rdf:resource="&fibo-fnd-info-info;WrittenInformation"/>
   </owl:Class>

   <owl:Class rdf:about="&fibo-fnd-info-info;WrittenInformation">
      <rdfs:label>written information</rdfs:label>
      <skos:definition>Some information which is written in some format (physical or electronic) and is or may be communicated in some way.</skos:definition>
      <rdfs:subClassOf rdf:resource="&fibo-fnd-info-info;Information"/>
      <rdfs:subClassOf rdf:resource="&fibo-uo-rl;IndependentThing"/>
   </owl:Class>

   <owl:Class rdf:about="&fibo-fnd-info-info;Information">
      <rdfs:label>information</rdfs:label>
      <rdfs:subClassOf rdf:resource="&fibo-uo-lat;Abstract"/>
   </owl:Class>

   <owl:Class rdf:about="&fibo-fnd-info-info;Name">
      <rdfs:label>name</rdfs:label>
      <rdfs:subClassOf rdf:resource="&fibo-uo-lat;ContinuantThing"/>
   </owl:Class>

   <owl:Class rdf:about="&fibo-fnd-info-info;StructuredName">
      <rdfs:label>structured name</rdfs:label>
      <skos:definition>A name with additional details besides simply being a string of text. This may include multilingual support or structuring of name content (as seen for example in financial securities names).</skos:definition>
      <rdfs:subClassOf rdf:resource="&fibo-fnd-info-info;Name"/>
   </owl:Class>


  <!--
    ///////////////////////////////////////////////////////////////////////////////////////
    //
    // Individuals
    //
    ///////////////////////////////////////////////////////////////////////////////////////
    -->


</rdf:RDF>