<?xml version="1.0"?>
<rdf:RDF xmlns="http://spec.edmcouncil.org/fibo/red/sec/debt/debt-foundations/parity-variants/"
     xml:base="http://spec.edmcouncil.org/fibo/red/sec/debt/debt-foundations/parity-variants/"
     xmlns:rdf="http://www.w3.org/1999/02/22-rdf-syntax-ns#"
     xmlns:owl="http://www.w3.org/2002/07/owl#"
     xmlns:xml="http://www.w3.org/XML/1998/namespace"
     xmlns:xsd="http://www.w3.org/2001/XMLSchema#"
     xmlns:skos="http://www.w3.org/2004/02/skos/core#"
     xmlns:rdfs="http://www.w3.org/2000/01/rdf-schema#">
    <owl:Ontology rdf:about="http://spec.edmcouncil.org/fibo/red/sec/debt/debt-foundations/parity-variants/"/>
    


    <!-- 
    ///////////////////////////////////////////////////////////////////////////////////////
    //
    // Annotation properties
    //
    ///////////////////////////////////////////////////////////////////////////////////////
     -->

    


    <!-- http://www.w3.org/2004/02/skos/core#definition -->

    <owl:AnnotationProperty rdf:about="http://www.w3.org/2004/02/skos/core#definition"/>
    


    <!-- 
    ///////////////////////////////////////////////////////////////////////////////////////
    //
    // Datatypes
    //
    ///////////////////////////////////////////////////////////////////////////////////////
     -->

    


    <!-- http://spec.edmcouncil.org/fibo/red/sec/debt/debt-foundations/parity-variants/DebtRelativeValueSelection -->

    <rdfs:Datatype rdf:about="http://spec.edmcouncil.org/fibo/red/sec/debt/debt-foundations/parity-variants/DebtRelativeValueSelection">
        <owl:equivalentClass>
            <rdfs:Datatype>
                <owl:oneOf>
                    <rdf:Description>
                        <rdf:type rdf:resource="http://www.w3.org/1999/02/22-rdf-syntax-ns#List"/>
                        <rdf:first rdf:datatype="http://www.w3.org/2001/XMLSchema#string">Discount</rdf:first>
                        <rdf:rest>
                            <rdf:Description>
                                <rdf:type rdf:resource="http://www.w3.org/1999/02/22-rdf-syntax-ns#List"/>
                                <rdf:first rdf:datatype="http://www.w3.org/2001/XMLSchema#string">Par</rdf:first>
                                <rdf:rest>
                                    <rdf:Description>
                                        <rdf:type rdf:resource="http://www.w3.org/1999/02/22-rdf-syntax-ns#List"/>
                                        <rdf:first rdf:datatype="http://www.w3.org/2001/XMLSchema#string">Premium</rdf:first>
                                        <rdf:rest rdf:resource="http://www.w3.org/1999/02/22-rdf-syntax-ns#nil"/>
                                    </rdf:Description>
                                </rdf:rest>
                            </rdf:Description>
                        </rdf:rest>
                    </rdf:Description>
                </owl:oneOf>
            </rdfs:Datatype>
        </owl:equivalentClass>
    </rdfs:Datatype>
    


    <!-- 
    ///////////////////////////////////////////////////////////////////////////////////////
    //
    // Data properties
    //
    ///////////////////////////////////////////////////////////////////////////////////////
     -->

    


    <!-- http://spec.edmcouncil.org/fibo/red/sec/debt/debt-foundations/parity-variants/valueAtIssue -->

    <owl:DatatypeProperty rdf:about="http://spec.edmcouncil.org/fibo/red/sec/debt/debt-foundations/parity-variants/valueAtIssue">
        <rdfs:range rdf:resource="http://spec.edmcouncil.org/fibo/red/sec/debt/debt-foundations/parity-variants/DebtRelativeValueSelection"/>
    </owl:DatatypeProperty>
    


    <!-- http://spec.edmcouncil.org/fibo/red/sec/debt/debt-foundations/parity-variants/valueAtIssue.1 -->

    <owl:DatatypeProperty rdf:about="http://spec.edmcouncil.org/fibo/red/sec/debt/debt-foundations/parity-variants/valueAtIssue.1">
        <rdfs:range rdf:resource="http://spec.edmcouncil.org/fibo/red/sec/debt/debt-foundations/parity-variants/DebtRelativeValueSelection"/>
    </owl:DatatypeProperty>
    


    <!-- http://spec.edmcouncil.org/fibo/red/sec/debt/debt-foundations/parity-variants/valueAtIssue.2 -->

    <owl:DatatypeProperty rdf:about="http://spec.edmcouncil.org/fibo/red/sec/debt/debt-foundations/parity-variants/valueAtIssue.2">
        <rdfs:range rdf:resource="http://spec.edmcouncil.org/fibo/red/sec/debt/debt-foundations/parity-variants/DebtRelativeValueSelection"/>
    </owl:DatatypeProperty>
    


    <!-- 
    ///////////////////////////////////////////////////////////////////////////////////////
    //
    // Classes
    //
    ///////////////////////////////////////////////////////////////////////////////////////
     -->

    


    <!-- http://spec.edmcouncil.org/fibo/red/sec/debt/debt-foundations/parity-variants/DiscountedInstrument -->

    <owl:Class rdf:about="http://spec.edmcouncil.org/fibo/red/sec/debt/debt-foundations/parity-variants/DiscountedInstrument"/>
    


    <!-- http://spec.edmcouncil.org/fibo/red/sec/debt/debt-foundations/parity-variants/ParInstrument -->

    <owl:Class rdf:about="http://spec.edmcouncil.org/fibo/red/sec/debt/debt-foundations/parity-variants/ParInstrument"/>
    


    <!-- http://spec.edmcouncil.org/fibo/red/sec/debt/debt-foundations/parity-variants/PremiumInstrument -->

    <owl:Class rdf:about="http://spec.edmcouncil.org/fibo/red/sec/debt/debt-foundations/parity-variants/PremiumInstrument"/>
    


    <!-- 
    ///////////////////////////////////////////////////////////////////////////////////////
    //
    // Annotations
    //
    ///////////////////////////////////////////////////////////////////////////////////////
     -->

    <rdf:Description rdf:about="http://spec.edmcouncil.org/fibo/red/sec/debt/debt-foundations/parity-variants/PremiumInstrument">
        <rdfs:label>premium instrument</rdfs:label>
    </rdf:Description>
    <rdf:Description rdf:about="http://spec.edmcouncil.org/fibo/red/sec/debt/debt-foundations/parity-variants/valueAtIssue.1">
        <rdfs:label>value at issue</rdfs:label>
        <skos:definition>The relative value at which the instrument is issued, namely par, premium or discount. For Par Instrument this is defined as Par.</skos:definition>
    </rdf:Description>
    <rdf:Description rdf:about="http://spec.edmcouncil.org/fibo/red/sec/debt/debt-foundations/parity-variants/valueAtIssue.2">
        <rdfs:label>value at issue</rdfs:label>
        <skos:definition>The relative value at which the instrument is issued, namely par, premium or discount. For Premium Instrument this is Premium.</skos:definition>
    </rdf:Description>
    <rdf:Description rdf:about="http://spec.edmcouncil.org/fibo/red/sec/debt/debt-foundations/parity-variants/valueAtIssue">
        <rdfs:label>value at issue</rdfs:label>
        <skos:definition>The relative value at which the instrument is issued, namely par, premium or discount. For Discount Instruments this is Discount.</skos:definition>
    </rdf:Description>
    <rdf:Description rdf:about="http://spec.edmcouncil.org/fibo/red/sec/debt/debt-foundations/parity-variants/DiscountedInstrument">
        <rdfs:label>discounted instrument</rdfs:label>
    </rdf:Description>
    <rdf:Description rdf:about="http://spec.edmcouncil.org/fibo/red/sec/debt/debt-foundations/parity-variants/DebtRelativeValueSelection">
        <skos:definition>A relative value of a debt instrument at some point in time. This is exhaustively either par value, a discount or a premium.</skos:definition>
    </rdf:Description>
    <rdf:Description rdf:about="http://spec.edmcouncil.org/fibo/red/sec/debt/debt-foundations/parity-variants/ParInstrument">
        <rdfs:label>par instrument</rdfs:label>
        <skos:definition>Instrument is issued at par. These instruments are issued at some face value and mature for a value equal to that face value plus interest.</skos:definition>
    </rdf:Description>
</rdf:RDF>



<!-- Generated by the OWL API (version 1.0.0-SNAPSHOT) http://owlapi.sourceforge.net -->

