<?xml version="1.0" encoding="UTF-8"?>
  
<!DOCTYPE rdf:RDF [
    <!ENTITY fibo-be-ptrx-jsp "http://spec.edmcouncil.org/fibo/red/be/partnerships-ext/jurisdiction-specific-partnerships/">
    <!ENTITY fibo-be-ptr-ptr "http://spec.edmcouncil.org/fibo/red/be/partnerships/partnerships/">
    <!ENTITY fibo-be-le-lp "http://spec.edmcouncil.org/fibo/red/be/legal-entities/legal-persons/">
    <!ENTITY fibo-be-oac-exec "http://spec.edmcouncil.org/fibo/red/be/ownership-and-control/executives/">
]>

<rdf:RDF xmlns:xsd="http://www.w3.org/2001/XMLSchema#"
         xmlns:sm="http://www.omg.org/techprocess/ab/SpecificationMetadata/"
         xmlns:xs="http://www.w3.org/2001/XMLSchema"
         xmlns:fibo-fnd-utl-av="http://www.omg.org/spec/EDMC-FIBO/FND/Utilities/AnnotationVocabulary/"
         xmlns:rdf="http://www.w3.org/1999/02/22-rdf-syntax-ns#"
         xmlns:rdfs="http://www.w3.org/2000/01/rdf-schema#"
         xmlns:owl="http://www.w3.org/2002/07/owl#"
         xmlns:skos="http://www.w3.org/2004/02/skos/core#"
         xmlns:dc="http://purl.org/dc/terms/"
         xml:base="http://spec.edmcouncil.org/fibo/red/be/partnerships-ext/jurisdiction-specific-partnerships/">

   <owl:Ontology rdf:about="http://spec.edmcouncil.org/fibo/red/be/partnerships-ext/jurisdiction-specific-partnerships/">
      <owl:imports rdf:resource="http://spec.edmcouncil.org/fibo/red/be/partnerships/partnerships/"/>
      <owl:imports rdf:resource="http://spec.edmcouncil.org/fibo/red/be/legal-entities/legal-persons/"/>
      <owl:imports rdf:resource="http://spec.edmcouncil.org/fibo/red/be/ownership-and-control/executives/"/>
   </owl:Ontology>


  <!--
    ///////////////////////////////////////////////////////////////////////////////////////
    //
    // Datatypes
    //
    ///////////////////////////////////////////////////////////////////////////////////////
    -->



  <!--
    ///////////////////////////////////////////////////////////////////////////////////////
    //
    // Object Properties
    //
    ///////////////////////////////////////////////////////////////////////////////////////
    -->


<owl:ObjectProperty rdf:about="&fibo-be-ptrx-jsp;hasAgent">
      <rdfs:label>has agent</rdfs:label>
      <skos:definition>The registered agent for the partnership.</skos:definition>
      <rdfs:subPropertyOf rdf:resource="&fibo-be-oac-exec;hasResponsibleParty"/>
      <rdfs:domain rdf:resource="&fibo-be-ptrx-jsp;LimitedLiabilityCompany_US_"/>
      <rdfs:range rdf:resource="&fibo-be-ptrx-jsp;LegallyIncorporatedPartershipRegisteredAgent"/>
   </owl:ObjectProperty>

   <owl:ObjectProperty rdf:about="&fibo-be-ptrx-jsp;registeredAgentIdentity">
      <rdfs:label>registered agent identity</rdfs:label>
      <skos:definition>The legal entity which is the Legally Incorporated Partnership Registered Agent</skos:definition>
      <rdfs:subPropertyOf rdf:resource="&fibo-be-oac-exec;responsiblePartyIdentity"/>
      <rdfs:domain rdf:resource="&fibo-be-ptrx-jsp;LegallyIncorporatedPartershipRegisteredAgent"/>
      <rdfs:range rdf:resource="&fibo-be-le-lp;NaturalPerson"/>
   </owl:ObjectProperty>


  <!--
    ///////////////////////////////////////////////////////////////////////////////////////
    //
    // Data Properties
    //
    ///////////////////////////////////////////////////////////////////////////////////////
    -->



  <!--
    ///////////////////////////////////////////////////////////////////////////////////////
    //
    // Annotation Properties
    //
    ///////////////////////////////////////////////////////////////////////////////////////
    -->



  <!--
    ///////////////////////////////////////////////////////////////////////////////////////
    //
    // Classes
    //
    ///////////////////////////////////////////////////////////////////////////////////////
    -->


<owl:Class rdf:about="&fibo-be-ptrx-jsp;LegallyIncorporatedPartershipRegisteredAgent">
      <rdfs:label>legally incorporated partership registered agent</rdfs:label>
      <skos:definition>The person - usually one of the members - who will act as the entity's registered agent or agent for service of process. This is the person designated to receive legal paprts in any legal action.</skos:definition>
      <rdfs:subClassOf rdf:resource="&fibo-be-oac-exec;ResponsibleParty"/>
   </owl:Class>

   <owl:Class rdf:about="&fibo-be-ptrx-jsp;LimitedLiabilityCompany_US_">
      <rdfs:label>limited liability company ( u s)</rdfs:label>
      <skos:definition>A company which is a legal entity and which gives participants limited liability, but has taxation status similar to a partnership.</skos:definition>
      <rdfs:subClassOf rdf:resource="&fibo-be-ptr-ptr;LegallyIncorporatedPartnership"/>
   </owl:Class>

   <owl:Class rdf:about="&fibo-be-ptrx-jsp;LimitedLiabilityPartnership_UK_">
      <rdfs:label>limited liability partnership ( u k)</rdfs:label>
      <skos:definition>British limited liability partnership (LLP) is a new form of legal business entity with limited liability. Limited liability partnerships are taxed as partnerships but in most other respects they are very similar to companies.</skos:definition>
   </owl:Class>

   <owl:Class rdf:about="&fibo-be-ptrx-jsp;LimitedLiabilityPartnership_US_">
      <rdfs:label>limited liability partnership ( u s)</rdfs:label>
   </owl:Class>

   <owl:Class rdf:about="&fibo-be-ptrx-jsp;LimitedPartnership_US_">
      <rdfs:label>limited partnership ( u s)</rdfs:label>
      <skos:definition>A business organization with one or more general partners, who manage the business and assume legal debts and obligations, and one or more limited partners, who are liable only to the extent of their investments.</skos:definition>
      <rdfs:subClassOf rdf:resource="&fibo-be-ptr-ptr;NonIncorporatedPartnership"/>
   </owl:Class>


  <!--
    ///////////////////////////////////////////////////////////////////////////////////////
    //
    // Individuals
    //
    ///////////////////////////////////////////////////////////////////////////////////////
    -->


</rdf:RDF>