<?xml version="1.0" encoding="UTF-8"?>
<!DOCTYPE rdf:RDF [
	<!ENTITY dct "http://purl.org/dc/terms/">
	<!ENTITY fibo-be-fct-pub "https://spec.edmcouncil.org/fibo/BE/FunctionalEntities/Publishers/">
	<!ENTITY fibo-fnd-acc-cur "https://spec.edmcouncil.org/fibo/FND/Accounting/CurrencyAmount/">
	<!ENTITY fibo-fnd-arr-arr "https://spec.edmcouncil.org/fibo/FND/Arrangements/Arrangements/">
	<!ENTITY fibo-fnd-dt-fd "https://spec.edmcouncil.org/fibo/FND/DatesAndTimes/FinancialDates/">
	<!ENTITY fibo-fnd-org-fm "https://spec.edmcouncil.org/fibo/FND/Organizations/FormalOrganizations/">
	<!ENTITY fibo-fnd-qt-qtu "https://spec.edmcouncil.org/fibo/FND/Quantities/QuantitiesAndUnits/">
	<!ENTITY fibo-fnd-rel-rel "https://spec.edmcouncil.org/fibo/FND/Relations/Relations/">
	<!ENTITY fibo-fnd-utl-alx "https://spec.edmcouncil.org/fibo/FND/Utilities/Analytics/">
	<!ENTITY fibo-fnd-utl-av "https://spec.edmcouncil.org/fibo/FND/Utilities/AnnotationVocabulary/">
	<!ENTITY fibo-fnd-utl-bt "https://spec.edmcouncil.org/fibo/FND/Utilities/BusinessFacingTypes/">
	<!ENTITY fibo-ind-ind-ind "https://spec.edmcouncil.org/fibo/IND/Indicators/Indicators/">
	<!ENTITY owl "http://www.w3.org/2002/07/owl#">
	<!ENTITY rdf "http://www.w3.org/1999/02/22-rdf-syntax-ns#">
	<!ENTITY rdfs "http://www.w3.org/2000/01/rdf-schema#">
	<!ENTITY skos "http://www.w3.org/2004/02/skos/core#">
	<!ENTITY sm "http://www.omg.org/techprocess/ab/SpecificationMetadata/">
	<!ENTITY xsd "http://www.w3.org/2001/XMLSchema#">
]>
<rdf:RDF xml:base="https://spec.edmcouncil.org/fibo/IND/Indicators/Indicators/"
	xmlns:dct="http://purl.org/dc/terms/"
	xmlns:fibo-be-fct-pub="https://spec.edmcouncil.org/fibo/BE/FunctionalEntities/Publishers/"
	xmlns:fibo-fnd-acc-cur="https://spec.edmcouncil.org/fibo/FND/Accounting/CurrencyAmount/"
	xmlns:fibo-fnd-arr-arr="https://spec.edmcouncil.org/fibo/FND/Arrangements/Arrangements/"
	xmlns:fibo-fnd-dt-fd="https://spec.edmcouncil.org/fibo/FND/DatesAndTimes/FinancialDates/"
	xmlns:fibo-fnd-org-fm="https://spec.edmcouncil.org/fibo/FND/Organizations/FormalOrganizations/"
	xmlns:fibo-fnd-qt-qtu="https://spec.edmcouncil.org/fibo/FND/Quantities/QuantitiesAndUnits/"
	xmlns:fibo-fnd-rel-rel="https://spec.edmcouncil.org/fibo/FND/Relations/Relations/"
	xmlns:fibo-fnd-utl-alx="https://spec.edmcouncil.org/fibo/FND/Utilities/Analytics/"
	xmlns:fibo-fnd-utl-av="https://spec.edmcouncil.org/fibo/FND/Utilities/AnnotationVocabulary/"
	xmlns:fibo-fnd-utl-bt="https://spec.edmcouncil.org/fibo/FND/Utilities/BusinessFacingTypes/"
	xmlns:fibo-ind-ind-ind="https://spec.edmcouncil.org/fibo/IND/Indicators/Indicators/"
	xmlns:owl="http://www.w3.org/2002/07/owl#"
	xmlns:rdf="http://www.w3.org/1999/02/22-rdf-syntax-ns#"
	xmlns:rdfs="http://www.w3.org/2000/01/rdf-schema#"
	xmlns:skos="http://www.w3.org/2004/02/skos/core#"
	xmlns:sm="http://www.omg.org/techprocess/ab/SpecificationMetadata/"
	xmlns:xsd="http://www.w3.org/2001/XMLSchema#">
	
	<owl:Ontology rdf:about="https://spec.edmcouncil.org/fibo/IND/Indicators/Indicators/">
		<rdfs:label>Indicators Ontology</rdfs:label>
		<dct:license rdf:resource="&sm;MITLicense"/>
		<sm:contentLanguage rdf:resource="http://www.omg.org/spec/ODM/"/>
		<sm:contentLanguage rdf:resource="http://www.w3.org/standards/techs/owl#w3c_all"/>
		<sm:copyright>Copyright (c) 2014-2017 EDM Council, Inc.
Copyright (c) 2014-2017 Object Management Group, Inc.</sm:copyright>
		<sm:dependsOn rdf:resource="https://spec.edmcouncil.org/fibo/BE/"/>
		<sm:dependsOn rdf:resource="https://spec.edmcouncil.org/fibo/FND/"/>
		<sm:fileAbbreviation>fibo-ind-ind-ind</sm:fileAbbreviation>
		<sm:fileAbstract>This ontology provides the concepts common to all market rates, indices and indicators; that is concepts descriptive of the numeric parameters themselves. These are modeled independently of the values they may take over time.</sm:fileAbstract>
		<sm:filename>Indicators.rdf</sm:filename>
		<rdfs:seeAlso rdf:resource="https://spec.edmcouncil.org/fibo/AboutTheEDMC-FIBOFamily/"/>
		<rdfs:seeAlso rdf:resource="https://spec.edmcouncil.org/fibo/IND/AboutIND/"/>
		<rdfs:seeAlso rdf:resource="https://spec.edmcouncil.org/fibo/IND/Indicators/AboutIndicators/"/>
		<owl:imports rdf:resource="https://spec.edmcouncil.org/fibo/BE/FunctionalEntities/Publishers/"/>
		<owl:imports rdf:resource="https://spec.edmcouncil.org/fibo/FND/Accounting/CurrencyAmount/"/>
		<owl:imports rdf:resource="https://spec.edmcouncil.org/fibo/FND/Arrangements/Arrangements/"/>
		<owl:imports rdf:resource="https://spec.edmcouncil.org/fibo/FND/DatesAndTimes/FinancialDates/"/>
		<owl:imports rdf:resource="https://spec.edmcouncil.org/fibo/FND/Organizations/FormalOrganizations/"/>
		<owl:imports rdf:resource="https://spec.edmcouncil.org/fibo/FND/Quantities/QuantitiesAndUnits/"/>
		<owl:imports rdf:resource="https://spec.edmcouncil.org/fibo/FND/Relations/Relations/"/>
		<owl:imports rdf:resource="https://spec.edmcouncil.org/fibo/FND/Utilities/Analytics/"/>
		<owl:imports rdf:resource="https://spec.edmcouncil.org/fibo/FND/Utilities/AnnotationVocabulary/"/>
		<owl:imports rdf:resource="https://spec.edmcouncil.org/fibo/FND/Utilities/BusinessFacingTypes/"/>
		<owl:versionIRI rdf:resource="https://spec.edmcouncil.org/fibo/IND/20170201/Indicators/Indicators/"/>
		<skos:changeNote>The https://spec.edmcouncil.org/fibo/IND/20140601/Indicators/Indicators.rdf version of this ontology was modified per the issue resolutions identified in the FIBO IND 1.0 FTF 1 report.</skos:changeNote>
		<skos:changeNote>The https://spec.edmcouncil.org/fibo/IND/20150501/Indicators/Indicators.rdf version of this ontology was modified per the issue resolutions identified in the FIBO IND 1.0 FTF 3 report, namely, to take advantage of content added via the FIBO FND 1.1 with respect to higher-level concepts of Rate, ExchangeRate, and InterestRate and revise the definition of TermStructure to better support concepts such as yield curves.</skos:changeNote>
		<skos:changeNote>The https://spec.edmcouncil.org/fibo/IND/20160801/Indicators/Indicators.rdf version of this ontology was modified per the issue resolutions identified in the FIBO IND 1.1 RTF report.</skos:changeNote>
		<fibo-fnd-utl-av:hasMaturityLevel rdf:resource="&fibo-fnd-utl-av;Release"/>
	</owl:Ontology>
	
	<owl:Class rdf:about="&fibo-ind-ind-ind;DailyAverageMarketRate">
		<rdfs:subClassOf rdf:resource="&fibo-ind-ind-ind;MarketRate"/>
		<rdfs:subClassOf>
			<owl:Restriction>
				<owl:onProperty rdf:resource="&fibo-ind-ind-ind;hasQuotationDate"/>
				<owl:onClass rdf:resource="&fibo-fnd-dt-fd;ExplicitDate"/>
				<owl:qualifiedCardinality rdf:datatype="&xsd;nonNegativeInteger">1</owl:qualifiedCardinality>
			</owl:Restriction>
		</rdfs:subClassOf>
		<rdfs:label>daily average market rate</rdfs:label>
		<skos:definition>a measure of the overall price level of a given rate, calculated as the sum of all values of the rates for a particular reference rate, foreign exchange rate, lending rate, or other market rate divided by the total number of rates collected over the course of a twenty-four (24) hour period for a specific date</skos:definition>
		<fibo-fnd-utl-av:adaptedFrom rdf:datatype="&xsd;anyURI">http://www.investopedia.com/terms/m/marketaverage.asp</fibo-fnd-utl-av:adaptedFrom>
	</owl:Class>
	
	<owl:Class rdf:about="&fibo-ind-ind-ind;EndOfDayMarketRate">
		<rdfs:subClassOf rdf:resource="&fibo-ind-ind-ind;MarketRate"/>
		<rdfs:subClassOf>
			<owl:Restriction>
				<owl:onProperty rdf:resource="&fibo-ind-ind-ind;hasQuotationDate"/>
				<owl:onClass rdf:resource="&fibo-fnd-dt-fd;ExplicitDate"/>
				<owl:qualifiedCardinality rdf:datatype="&xsd;nonNegativeInteger">1</owl:qualifiedCardinality>
			</owl:Restriction>
		</rdfs:subClassOf>
		<rdfs:label>end-of-day market rate</rdfs:label>
		<skos:definition>a measure of the price level (value) of a given market rate of the end of the business day for a specific date</skos:definition>
	</owl:Class>
	
	<owl:Class rdf:about="&fibo-ind-ind-ind;FinancialInformationPublisher">
		<rdfs:subClassOf rdf:resource="&fibo-be-fct-pub;Publisher"/>
		<rdfs:subClassOf>
			<owl:Restriction>
				<owl:onProperty rdf:resource="&fibo-be-fct-pub;publishes"/>
				<owl:onClass rdf:resource="&fibo-ind-ind-ind;PublishedFinancialInformation"/>
				<owl:minQualifiedCardinality rdf:datatype="&xsd;nonNegativeInteger">0</owl:minQualifiedCardinality>
			</owl:Restriction>
		</rdfs:subClassOf>
		<rdfs:subClassOf>
			<owl:Restriction>
				<owl:onProperty rdf:resource="&fibo-fnd-rel-rel;hasIdentity"/>
				<owl:someValuesFrom rdf:resource="&fibo-fnd-org-fm;FormalOrganization"/>
			</owl:Restriction>
		</rdfs:subClassOf>
		<rdfs:label>financial information publisher</rdfs:label>
		<skos:definition>a formal organization acting as a publisher or provider of information related to the financial markets or of interest to financial market participants such as information on economies</skos:definition>
	</owl:Class>
	
	<owl:Class rdf:about="&fibo-ind-ind-ind;MarketRate">
		<rdfs:subClassOf rdf:resource="&fibo-fnd-qt-qtu;Rate"/>
		<rdfs:subClassOf rdf:resource="&fibo-ind-ind-ind;PublishedFinancialInformation"/>
		<rdfs:subClassOf>
			<owl:Restriction>
				<owl:onProperty rdf:resource="&fibo-ind-ind-ind;hasQuotationDate"/>
				<owl:allValuesFrom rdf:resource="&fibo-fnd-dt-fd;Date"/>
			</owl:Restriction>
		</rdfs:subClassOf>
		<rdfs:subClassOf>
			<owl:Restriction>
				<owl:onProperty rdf:resource="&fibo-ind-ind-ind;hasQuotationDateTime"/>
				<owl:allValuesFrom rdf:resource="&fibo-fnd-dt-fd;DateTime"/>
			</owl:Restriction>
		</rdfs:subClassOf>
		<rdfs:label xml:lang="en">market rate</rdfs:label>
		<skos:definition>a measure that is also published financial information providing a rate used to measure market trends for a set of instruments (S&amp;P500, NASDAQ composite, 30 day CD) or that describes the economic climate for an industry (Dow Jones Industrial Average (DJIA), H&amp;Q Growth Technologies) and/or political region (LIBOR, Prime)</skos:definition>
		<skos:example>Financial market rates include, but are not limited to reference rates, foreign exchange rates, lending rates, bankers&apos; acceptance rates, and so forth.</skos:example>
		<skos:scopeNote>Market rates include but may not be limited to the following:
(1) Index: Statistical composite that measures changes in the economy or in financial markets, often expressed in percentage changes from a base year or from the previous month
(2) Money Rate: Benchmark or guideline for interest rates determined by central banks or economical climate as a whole
(3) Bankers&apos; Acceptance Rate: Benchmark reflecting market fluctuations of Bankers&apos; Acceptance issued instruments                
(4) Commercial Paper Rate: Benchmark reflecting market fluctuations of Commercial Paper issued instruments        
(5) Certificate of Deposit Rate: Benchmark reflecting market fluctuations of Certificate of Deposit issued instruments                
(6) Interbank Rate                                                
(7) Prime                        
(8) Time Deposit Rate: Benchmark reflecting market fluctuations of Deposit/Redeposit issued instruments</skos:scopeNote>
		<skos:scopeNote>known collectively (in the CFI Standard) as referential instruments</skos:scopeNote>
	</owl:Class>
	
	<owl:Class rdf:about="&fibo-ind-ind-ind;MarketSpread">
		<rdfs:subClassOf rdf:resource="&fibo-fnd-utl-alx;StatisticalMeasure"/>
		<rdfs:subClassOf>
			<owl:Restriction>
				<owl:onProperty rdf:resource="&fibo-fnd-utl-alx;hasOperand"/>
				<owl:onClass rdf:resource="&fibo-ind-ind-ind;MarketRate"/>
				<owl:qualifiedCardinality rdf:datatype="&xsd;nonNegativeInteger">2</owl:qualifiedCardinality>
			</owl:Restriction>
		</rdfs:subClassOf>
		<rdfs:label>market spread</rdfs:label>
		<skos:definition>a statistical measure providing the difference (or spread) between two market rates</skos:definition>
	</owl:Class>
	
	<owl:Class rdf:about="&fibo-ind-ind-ind;PriceStructure">
		<rdfs:subClassOf rdf:resource="&fibo-fnd-arr-arr;StructuredCollection"/>
		<rdfs:subClassOf>
			<owl:Restriction>
				<owl:onProperty rdf:resource="&fibo-fnd-rel-rel;comprises"/>
				<owl:someValuesFrom rdf:resource="&fibo-ind-ind-ind;QuotedPrice"/>
			</owl:Restriction>
		</rdfs:subClassOf>
		<rdfs:label>price structure</rdfs:label>
		<skos:definition>a structured collection of quoted prices, such as market prices for some index or security, such that volatility may be constructed for the structure</skos:definition>
	</owl:Class>
	
	<owl:Class rdf:about="&fibo-ind-ind-ind;PublishedFinancialInformation">
		<rdfs:subClassOf rdf:resource="&fibo-be-fct-pub;Publication"/>
		<rdfs:subClassOf>
			<owl:Restriction>
				<owl:onProperty rdf:resource="&fibo-be-fct-pub;hasPublisher"/>
				<owl:allValuesFrom rdf:resource="&fibo-ind-ind-ind;FinancialInformationPublisher"/>
			</owl:Restriction>
		</rdfs:subClassOf>
		<rdfs:label>published financial information</rdfs:label>
		<skos:definition>published information made available by a financial information publisher</skos:definition>
	</owl:Class>
	
	<owl:Class rdf:about="&fibo-ind-ind-ind;QuotedPrice">
		<rdfs:subClassOf rdf:resource="&fibo-fnd-acc-cur;MonetaryPrice"/>
		<rdfs:subClassOf rdf:resource="&fibo-ind-ind-ind;PublishedFinancialInformation"/>
		<rdfs:subClassOf>
			<owl:Restriction>
				<owl:onProperty rdf:resource="&fibo-ind-ind-ind;hasQuotationDate"/>
				<owl:onClass rdf:resource="&fibo-fnd-dt-fd;Date"/>
				<owl:qualifiedCardinality rdf:datatype="&xsd;nonNegativeInteger">1</owl:qualifiedCardinality>
			</owl:Restriction>
		</rdfs:subClassOf>
		<rdfs:label>quoted price</rdfs:label>
		<skos:definition>a monetary price quoted by some publisher on a given date</skos:definition>
	</owl:Class>
	
	<owl:Class rdf:about="&fibo-ind-ind-ind;StructuredCollection">
		<rdfs:subClassOf rdf:resource="&fibo-fnd-arr-arr;Collection"/>
		<rdfs:label>structured collection</rdfs:label>
		<owl:deprecated rdf:datatype="&xsd;boolean">true</owl:deprecated>
		<skos:definition>a collection that has a clearly defined structure or organization</skos:definition>
	</owl:Class>
	
	<owl:Class rdf:about="&fibo-ind-ind-ind;TermStructure">
		<rdfs:subClassOf rdf:resource="&fibo-fnd-arr-arr;StructuredCollection"/>
		<rdfs:subClassOf>
			<owl:Restriction>
				<owl:onProperty rdf:resource="&fibo-fnd-rel-rel;hasPart"/>
				<owl:someValuesFrom rdf:resource="&fibo-ind-ind-ind;MarketRate"/>
			</owl:Restriction>
		</rdfs:subClassOf>
		<rdfs:label>term structure</rdfs:label>
		<skos:definition>a structured collection of rates, such as interest rates, or bond yields with different terms to maturity, such that a yield curve may be constructed for the structure</skos:definition>
		<skos:editorialNote>Term structure refers to a set of discrete points; elements are ordered by time. Restrictions on the rate (see above) and a point in time, paired together, and then ordered in a structured collection is how this should ultimately be modeled.  Then the concept of yield curve would be a child of term structure, for calculation of net present value, for example.</skos:editorialNote>
		<skos:scopeNote>Term Structure has been modeled with reference to MarketRate generally, which incorporates more kinds of rate than would normally be included in a term structure. Term structures consist of two or more of something with some time to maturity, typically debt instruments or interest rates. Currency exchange rates may in principle be grouped in a term structure as forward rates. For this specification, debt instruments are not in scope, so these are not included in the current scope of this TermStructure concept.</skos:scopeNote>
		<fibo-fnd-utl-av:adaptedFrom rdf:datatype="&xsd;anyURI">http://www.investopedia.com/terms/t/termstructure.asp</fibo-fnd-utl-av:adaptedFrom>
		<fibo-fnd-utl-av:explanatoryNote>The term structure reflects expectations of market participants about future changes in interest rates and their assessment of monetary policy conditions.</fibo-fnd-utl-av:explanatoryNote>
	</owl:Class>
	
	<owl:Class rdf:about="&fibo-ind-ind-ind;Volatility">
		<rdfs:subClassOf rdf:resource="&fibo-fnd-utl-alx;Expression"/>
		<rdfs:subClassOf rdf:resource="&fibo-fnd-utl-alx;StatisticalMeasure"/>
		<rdfs:subClassOf>
			<owl:Restriction>
				<owl:onProperty rdf:resource="&fibo-fnd-dt-fd;hasDatePeriod"/>
				<owl:someValuesFrom rdf:resource="&fibo-fnd-dt-fd;DatePeriod"/>
			</owl:Restriction>
		</rdfs:subClassOf>
		<rdfs:subClassOf>
			<owl:Restriction>
				<owl:onProperty rdf:resource="&fibo-fnd-utl-alx;hasArgument"/>
				<owl:someValuesFrom rdf:resource="&fibo-ind-ind-ind;PriceStructure"/>
			</owl:Restriction>
		</rdfs:subClassOf>
		<rdfs:label>volatility</rdfs:label>
		<skos:definition>a statistical measure of the rate of change in pricing for a given security or market index</skos:definition>
		<skos:editorialNote>Volatility is modeled here as a structured collection, comprised of a series of individual prices of something (a security, index, etc., typically quoted prices), dates, and the source for those prices for some overall period of time</skos:editorialNote>
		<fibo-fnd-utl-av:adaptedFrom rdf:datatype="&xsd;anyURI">OptionsEducation.org</fibo-fnd-utl-av:adaptedFrom>
		<fibo-fnd-utl-av:explanatoryNote>Volatility can be determined using the standard deviation or variance among prices for the security or market index over some period of time. For a specific security, volatility may measure the amount and frequency in rapid price fluctuation. It is computed as the annualized standard deviation of the percentage change in a security&apos;s daily price.</fibo-fnd-utl-av:explanatoryNote>
	</owl:Class>
	
	<owl:ObjectProperty rdf:about="&fibo-ind-ind-ind;hasQuotationDate">
		<rdfs:subPropertyOf rdf:resource="&fibo-fnd-dt-fd;hasDate"/>
		<rdfs:label>has quotation date</rdfs:label>
		<rdfs:range rdf:resource="&fibo-fnd-dt-fd;Date"/>
		<skos:definition>indicates the quotation date for a given market rate or indicator</skos:definition>
		<fibo-fnd-utl-av:explanatoryNote>Typically this property reflects a daily average or end of day quote.</fibo-fnd-utl-av:explanatoryNote>
	</owl:ObjectProperty>
	
	<owl:ObjectProperty rdf:about="&fibo-ind-ind-ind;hasQuotationDateTime">
		<rdfs:subPropertyOf rdf:resource="&fibo-fnd-dt-fd;hasDateTime"/>
		<rdfs:label>has quotation date and time</rdfs:label>
		<rdfs:range rdf:resource="&fibo-fnd-dt-fd;DateTime"/>
		<skos:definition>indicates the quotation date and time for a given market rate or indicator</skos:definition>
	</owl:ObjectProperty>
	
	<owl:ObjectProperty rdf:about="&fibo-ind-ind-ind;isVolatilityOf">
		<rdfs:subPropertyOf rdf:resource="&fibo-fnd-rel-rel;appliesTo"/>
		<rdfs:label>is volatility of</rdfs:label>
		<rdfs:domain rdf:resource="&fibo-ind-ind-ind;Volatility"/>
		<rdfs:range rdf:resource="&fibo-ind-ind-ind;MarketRate"/>
		<skos:definition>indicates the market rate to which the volatility measure applies and of which it is a measure</skos:definition>
	</owl:ObjectProperty>

</rdf:RDF>