<?xml version="1.0" encoding="UTF-8"?>
<!DOCTYPE rdf:RDF [
	<!ENTITY dct "http://purl.org/dc/terms/">
	<!ENTITY fibo-be-le-fbo "https://spec.edmcouncil.org/fibo/ontology/BE/LegalEntities/FormalBusinessOrganizations/">
	<!ENTITY fibo-be-le-lp "https://spec.edmcouncil.org/fibo/ontology/BE/LegalEntities/LegalPersons/">
	<!ENTITY fibo-be-oac-cpty "https://spec.edmcouncil.org/fibo/ontology/BE/OwnershipAndControl/ControlParties/">
	<!ENTITY fibo-be-oac-opty "https://spec.edmcouncil.org/fibo/ontology/BE/OwnershipAndControl/OwnershipParties/">
	<!ENTITY fibo-fnd-agr-ctr "https://spec.edmcouncil.org/fibo/ontology/FND/Agreements/Contracts/">
	<!ENTITY fibo-fnd-law-cor "https://spec.edmcouncil.org/fibo/ontology/FND/Law/LegalCore/">
	<!ENTITY fibo-fnd-oac-ctl "https://spec.edmcouncil.org/fibo/ontology/FND/OwnershipAndControl/Control/">
	<!ENTITY fibo-fnd-org-fm "https://spec.edmcouncil.org/fibo/ontology/FND/Organizations/FormalOrganizations/">
	<!ENTITY fibo-fnd-pty-pty "https://spec.edmcouncil.org/fibo/ontology/FND/Parties/Parties/">
	<!ENTITY fibo-fnd-pty-rl "https://spec.edmcouncil.org/fibo/ontology/FND/Parties/Roles/">
	<!ENTITY fibo-fnd-rel-rel "https://spec.edmcouncil.org/fibo/ontology/FND/Relations/Relations/">
	<!ENTITY fibo-fnd-utl-av "https://spec.edmcouncil.org/fibo/ontology/FND/Utilities/AnnotationVocabulary/">
	<!ENTITY lcc-lr "https://www.omg.org/spec/LCC/Languages/LanguageRepresentation/">
	<!ENTITY owl "http://www.w3.org/2002/07/owl#">
	<!ENTITY rdf "http://www.w3.org/1999/02/22-rdf-syntax-ns#">
	<!ENTITY rdfs "http://www.w3.org/2000/01/rdf-schema#">
	<!ENTITY skos "http://www.w3.org/2004/02/skos/core#">
	<!ENTITY sm "http://www.omg.org/techprocess/ab/SpecificationMetadata/">
	<!ENTITY xsd "http://www.w3.org/2001/XMLSchema#">
]>
<rdf:RDF xml:base="https://spec.edmcouncil.org/fibo/ontology/BE/OwnershipAndControl/ControlParties/"
	xmlns:dct="http://purl.org/dc/terms/"
	xmlns:fibo-be-le-fbo="https://spec.edmcouncil.org/fibo/ontology/BE/LegalEntities/FormalBusinessOrganizations/"
	xmlns:fibo-be-le-lp="https://spec.edmcouncil.org/fibo/ontology/BE/LegalEntities/LegalPersons/"
	xmlns:fibo-be-oac-cpty="https://spec.edmcouncil.org/fibo/ontology/BE/OwnershipAndControl/ControlParties/"
	xmlns:fibo-be-oac-opty="https://spec.edmcouncil.org/fibo/ontology/BE/OwnershipAndControl/OwnershipParties/"
	xmlns:fibo-fnd-agr-ctr="https://spec.edmcouncil.org/fibo/ontology/FND/Agreements/Contracts/"
	xmlns:fibo-fnd-law-cor="https://spec.edmcouncil.org/fibo/ontology/FND/Law/LegalCore/"
	xmlns:fibo-fnd-oac-ctl="https://spec.edmcouncil.org/fibo/ontology/FND/OwnershipAndControl/Control/"
	xmlns:fibo-fnd-org-fm="https://spec.edmcouncil.org/fibo/ontology/FND/Organizations/FormalOrganizations/"
	xmlns:fibo-fnd-pty-pty="https://spec.edmcouncil.org/fibo/ontology/FND/Parties/Parties/"
	xmlns:fibo-fnd-pty-rl="https://spec.edmcouncil.org/fibo/ontology/FND/Parties/Roles/"
	xmlns:fibo-fnd-rel-rel="https://spec.edmcouncil.org/fibo/ontology/FND/Relations/Relations/"
	xmlns:fibo-fnd-utl-av="https://spec.edmcouncil.org/fibo/ontology/FND/Utilities/AnnotationVocabulary/"
	xmlns:lcc-lr="https://www.omg.org/spec/LCC/Languages/LanguageRepresentation/"
	xmlns:owl="http://www.w3.org/2002/07/owl#"
	xmlns:rdf="http://www.w3.org/1999/02/22-rdf-syntax-ns#"
	xmlns:rdfs="http://www.w3.org/2000/01/rdf-schema#"
	xmlns:skos="http://www.w3.org/2004/02/skos/core#"
	xmlns:sm="http://www.omg.org/techprocess/ab/SpecificationMetadata/"
	xmlns:xsd="http://www.w3.org/2001/XMLSchema#">
	
	<owl:Ontology rdf:about="https://spec.edmcouncil.org/fibo/ontology/BE/OwnershipAndControl/ControlParties/">
		<rdfs:label>Control Parties Ontology</rdfs:label>
		<dct:abstract>This ontology defines concepts relating to types of controlling parties. The concepts defined here are party in role concepts, which define the nature of some entity such as an organization or a legal person, in some role such as that of owning a controlling interest in the entity or of controlling that entity. These roles are defined in terms of the types of control enjoyed by the party, for example de facto or de jure control. An important feature of this ontology is the distinction between the holding of a controlling interest (such as voting shares), and the de facto existence of control of one body by another as asserted in company filings or as a conclusion drawn from computational analysis of controlling interests.</dct:abstract>
		<dct:license rdf:datatype="&xsd;anyURI">http://opensource.org/licenses/MIT</dct:license>
		<sm:contentLanguage rdf:datatype="&xsd;anyURI">http://www.w3.org/standards/techs/owl#w3c_all</sm:contentLanguage>
		<sm:copyright>Copyright (c) 2013-2020 EDM Council, Inc.</sm:copyright>
		<sm:copyright>Copyright (c) 2013-2020 Object Management Group, Inc.</sm:copyright>
		<sm:dependsOn rdf:datatype="&xsd;anyURI">https://spec.edmcouncil.org/fibo/ontology/BE/LegalEntities/FormalBusinessOrganizations/</sm:dependsOn>
		<sm:dependsOn rdf:datatype="&xsd;anyURI">https://spec.edmcouncil.org/fibo/ontology/BE/LegalEntities/LegalPersons/</sm:dependsOn>
		<sm:dependsOn rdf:datatype="&xsd;anyURI">https://spec.edmcouncil.org/fibo/ontology/BE/OwnershipAndControl/OwnershipParties/</sm:dependsOn>
		<sm:dependsOn rdf:datatype="&xsd;anyURI">https://spec.edmcouncil.org/fibo/ontology/FND/</sm:dependsOn>
		<sm:fileAbbreviation>fibo-be-oac-cpty</sm:fileAbbreviation>
		<sm:filename>ControlParties.rdf</sm:filename>
		<owl:imports rdf:resource="https://spec.edmcouncil.org/fibo/ontology/BE/LegalEntities/FormalBusinessOrganizations/"/>
		<owl:imports rdf:resource="https://spec.edmcouncil.org/fibo/ontology/BE/LegalEntities/LegalPersons/"/>
		<owl:imports rdf:resource="https://spec.edmcouncil.org/fibo/ontology/BE/OwnershipAndControl/OwnershipParties/"/>
		<owl:imports rdf:resource="https://spec.edmcouncil.org/fibo/ontology/FND/Agreements/Contracts/"/>
		<owl:imports rdf:resource="https://spec.edmcouncil.org/fibo/ontology/FND/Law/LegalCore/"/>
		<owl:imports rdf:resource="https://spec.edmcouncil.org/fibo/ontology/FND/Organizations/FormalOrganizations/"/>
		<owl:imports rdf:resource="https://spec.edmcouncil.org/fibo/ontology/FND/OwnershipAndControl/Control/"/>
		<owl:imports rdf:resource="https://spec.edmcouncil.org/fibo/ontology/FND/Parties/Parties/"/>
		<owl:imports rdf:resource="https://spec.edmcouncil.org/fibo/ontology/FND/Parties/Roles/"/>
		<owl:imports rdf:resource="https://spec.edmcouncil.org/fibo/ontology/FND/Relations/Relations/"/>
		<owl:imports rdf:resource="https://spec.edmcouncil.org/fibo/ontology/FND/Utilities/AnnotationVocabulary/"/>
		<owl:imports rdf:resource="https://www.omg.org/spec/LCC/Languages/LanguageRepresentation/"/>
		<owl:versionIRI rdf:resource="https://spec.edmcouncil.org/fibo/ontology/BE/20200201/OwnershipAndControl/ControlParties/"/>
		<skos:changeNote>The https://spec.edmcouncil.org/fibo/ontology/BE/20131101/OwnershipAndControl/ControlParties.rdf version of this ontology was modified per the issue resolutions identified in the FIBO BE 1.0 FTF report.</skos:changeNote>
		<skos:changeNote>The https://spec.edmcouncil.org/fibo/ontology/BE/20160201/OwnershipAndControl/ControlParties.rdf version of this ontology was modified per the FIBO 2.0 RFC to add missing labels and definitions, eliminate references to BusinessFacingTypes, etc.</skos:changeNote>
		<skos:changeNote>The https://spec.edmcouncil.org/fibo/ontology/BE/20180801/OwnershipAndControl/ControlParties.rdf version of this ontology was modified as a part of a simplification strategy for the organizational class hierarchy and to correct reasoning anomalies.</skos:changeNote>
		<skos:changeNote>The https://spec.edmcouncil.org/fibo/ontology/BE/20190101/OwnershipAndControl/ControlParties.rdf version of this ontology was modified to eliminate duplication of concepts with LCC.</skos:changeNote>
		<fibo-fnd-utl-av:hasMaturityLevel rdf:resource="&fibo-fnd-utl-av;Release"/>
	</owl:Ontology>
	
	<owl:Class rdf:about="&fibo-be-oac-cpty;COCOBondholder">
		<rdfs:subClassOf rdf:resource="&fibo-be-oac-cpty;PartyHoldingSomeOptionForControl"/>
		<rdfs:label>COCO bondholder</rdfs:label>
		<skos:definition>Holder of bank bonds which convert to equity holdings in a bank.</skos:definition>
		<skos:editorialNote>These equity holdings, when they exist, will confer upon the holder some de jure controlling interest in the issuing entity.</skos:editorialNote>
	</owl:Class>
	
	<owl:Class rdf:about="&fibo-be-oac-cpty;ConstitutionalContractualControl">
		<rdfs:subClassOf rdf:resource="&fibo-be-oac-cpty;ConstitutionalDeJureControl"/>
		<rdfs:subClassOf rdf:resource="&fibo-be-oac-cpty;ContractualControl"/>
		<rdfs:subClassOf>
			<owl:Restriction>
				<owl:onProperty rdf:resource="&fibo-fnd-rel-rel;isConferredBy"/>
				<owl:someValuesFrom rdf:resource="&fibo-be-le-fbo;OrganizationCoveringAgreement"/>
			</owl:Restriction>
		</rdfs:subClassOf>
		<rdfs:label>constitutional contractual control</rdfs:label>
		<skos:definition>Some control set out in some contract among the principals of an organization.</skos:definition>
		<skos:editorialNote>This distinguishes this control from control conferred by contracts with third parties, for example in relation to third party guarantees or similar. This combines all forms of constitutional control in one set of terms under Constitutional De Jure Control.</skos:editorialNote>
	</owl:Class>
	
	<owl:Class rdf:about="&fibo-be-oac-cpty;ConstitutionalDeJureControl">
		<rdfs:subClassOf rdf:resource="&fibo-be-oac-cpty;DeJureControllingInterest"/>
		<rdfs:label>constitutional de jure control</rdfs:label>
		<skos:definition>Control which is based in some instrument which has constitutional standing (is constitutive of the entity) such as voting shares, general partner equity etc.</skos:definition>
	</owl:Class>
	
	<owl:Class rdf:about="&fibo-be-oac-cpty;ContractualControl">
		<rdfs:subClassOf rdf:resource="&fibo-fnd-oac-ctl;ControllingCapacity"/>
		<rdfs:subClassOf>
			<owl:Restriction>
				<owl:onProperty rdf:resource="&fibo-fnd-rel-rel;isConferredBy"/>
				<owl:someValuesFrom rdf:resource="&fibo-fnd-agr-ctr;Contract"/>
			</owl:Restriction>
		</rdfs:subClassOf>
		<rdfs:label>contractual control</rdfs:label>
		<skos:definition>Control vested in an entity by virtue of the terms in some contract between that entity and others.</skos:definition>
		<skos:editorialNote>See SME REview note of 16 Jan 2013: Percentage mechanism (in contracts etc.) would be factored in. Hence percentages as contractual terms. For instance an option to exercise which would give another 5 percent control. So there is percentage control with or without share ownership. Example: In a partnership this might be in the Partnership Agreement, which would identify beneficial ownership and control as potentially 2 distinct things. Contract can say anything. Implications: This means that there are percentages of de jure control based in contract, similar to those based in constitutional instruments (shares, General Partner equity). The concepts of Parent, Siinificant Part Owner etc. can then potentially be defined int erms of the percentages of all applicable instruments by which control may be formally defined.</skos:editorialNote>
	</owl:Class>
	
	<owl:Class rdf:about="&fibo-be-oac-cpty;ContractualControllingParty">
		<rdfs:subClassOf rdf:resource="&fibo-be-oac-cpty;DeJureControllingInterestParty"/>
		<rdfs:subClassOf>
			<owl:Restriction>
				<owl:onProperty rdf:resource="&fibo-be-oac-cpty;holdsSomeMeansOf"/>
				<owl:someValuesFrom rdf:resource="&fibo-be-oac-cpty;ContractualControl"/>
			</owl:Restriction>
		</rdfs:subClassOf>
		<rdfs:label>contractual controlling party</rdfs:label>
		<skos:definition>A party which exercises some control which is set out in some contract.</skos:definition>
		<skos:editorialNote>This is as distinct from control set out in some constitutional instrument e.g. voting shares ownership or general partner equity.</skos:editorialNote>
	</owl:Class>
	
	<owl:Class rdf:about="&fibo-be-oac-cpty;ControlledParty">
		<rdfs:subClassOf rdf:resource="&fibo-fnd-pty-pty;PartyInRole"/>
		<rdfs:subClassOf>
			<owl:Restriction>
				<owl:onProperty rdf:resource="&fibo-fnd-pty-rl;isPlayedBy"/>
				<owl:someValuesFrom>
					<owl:Restriction>
						<owl:onProperty rdf:resource="&fibo-be-oac-cpty;isControlledToSomeDegreeBy"/>
						<owl:someValuesFrom rdf:resource="&fibo-fnd-oac-ctl;ControllingParty"/>
					</owl:Restriction>
				</owl:someValuesFrom>
			</owl:Restriction>
		</rdfs:subClassOf>
		<rdfs:label>controlled party</rdfs:label>
		<skos:definition>Some party which is controlled in some way and to some degree by some other party.</skos:definition>
		<skos:editorialNote>Scope Note: Parties, since they stand in roles, will have relationships among them which correspond to the reciprocals of the roles they stand in. In this case, controls and controlled by.</skos:editorialNote>
	</owl:Class>
	
	<owl:Class rdf:about="&fibo-be-oac-cpty;ControllingAlliance">
		<rdfs:subClassOf rdf:resource="&fibo-fnd-org-fm;Group"/>
		<rdfs:label>controlling alliance</rdfs:label>
		<skos:definition>Some group of entities which have formed some alliance or agreement in terms of which they jointly exercise control over some entity.</skos:definition>
		<skos:editorialNote>The types of entity which may enter into such an alliance are the same types of entity as may exercise control in their own right, i.e. independent parties (that is a logical union of natural persons, legal persons and formal organizations).</skos:editorialNote>
	</owl:Class>
	
	<owl:Class rdf:about="&fibo-be-oac-cpty;ControllingInterestOptionHolder">
		<rdfs:subClassOf rdf:resource="&fibo-be-oac-cpty;PartyHoldingSomeOptionForControl"/>
		<rdfs:label>controlling interest option holder</rdfs:label>
		<skos:definition>A party which holds some option which may be exercised to confer on that party some de jure controlling interest at some time in the future and at the discretion of that holder.</skos:definition>
	</owl:Class>
	
	<owl:Class rdf:about="&fibo-be-oac-cpty;ControllingInterestParty">
		<rdfs:subClassOf rdf:resource="&fibo-fnd-oac-ctl;ControllingParty"/>
		<rdfs:subClassOf>
			<owl:Restriction>
				<owl:onProperty rdf:resource="&fibo-be-oac-cpty;holdsSomeMeansOf"/>
				<owl:someValuesFrom rdf:resource="&fibo-fnd-oac-ctl;ControllingCapacity"/>
			</owl:Restriction>
		</rdfs:subClassOf>
		<rdfs:label>controlling interest party</rdfs:label>
		<skos:definition>Some party which holds some form of controlling interest in some other party in some context.</skos:definition>
		<skos:editorialNote>This controlling interest inevitably means that the party exercises some form of control, however the precise degree and nature of that control is dependent on many factors, and so is defined as a separate party role (which may and usually is fulfilled by the same entity).</skos:editorialNote>
	</owl:Class>
	
	<owl:Class rdf:about="&fibo-be-oac-cpty;ControllingLeverageParty">
		<rdfs:subClassOf rdf:resource="&fibo-be-oac-cpty;DeFactoControllingInterestParty"/>
		<rdfs:subClassOf>
			<owl:Restriction>
				<owl:onProperty rdf:resource="&fibo-be-oac-cpty;holdsSomeMeansOf"/>
				<owl:someValuesFrom rdf:resource="&fibo-be-oac-cpty;InvestmentBasedDeFactoControl"/>
			</owl:Restriction>
		</rdfs:subClassOf>
		<rdfs:label>controlling leverage party</rdfs:label>
		<skos:definition>A party which exercises control as a result of some investment in an equity.</skos:definition>
		<skos:editorialNote>Any large investor may have some degree of de facto control.</skos:editorialNote>
	</owl:Class>
	
	<owl:Class rdf:about="&fibo-be-oac-cpty;CourtAppointedControl">
		<rdfs:subClassOf rdf:resource="&fibo-fnd-oac-ctl;ControllingCapacity"/>
		<rdfs:subClassOf>
			<owl:Restriction>
				<owl:onProperty rdf:resource="&fibo-fnd-rel-rel;isConferredBy"/>
				<owl:allValuesFrom rdf:resource="&fibo-fnd-law-cor;CourtOfLaw"/>
			</owl:Restriction>
		</rdfs:subClassOf>
		<rdfs:label>court appointed control</rdfs:label>
		<skos:definition>Control conferred on some entity by act of some court, for example in the context of receivership.</skos:definition>
	</owl:Class>
	
	<owl:Class rdf:about="&fibo-be-oac-cpty;DeFactoControllingInterestParty">
		<rdfs:subClassOf rdf:resource="&fibo-be-oac-cpty;ControllingInterestParty"/>
		<rdfs:subClassOf>
			<owl:Restriction>
				<owl:onProperty rdf:resource="&fibo-be-oac-cpty;holdsSomeMeansOf"/>
				<owl:someValuesFrom rdf:resource="&fibo-fnd-oac-ctl;DeFactoControl"/>
			</owl:Restriction>
		</rdfs:subClassOf>
		<rdfs:label>de facto controlling interest party</rdfs:label>
		<skos:definition>A party which exercises some control over an entity other than via some constitutional instrument such as shares.</skos:definition>
		<skos:example>a silent partner, i.e. where someone has made a large investment, which is bilateral (not part of the constitutional framework of the company)</skos:example>
		<skos:scopeNote>divides further into financial leverage via loans; non fiscal types of leverage (influence)</skos:scopeNote>
	</owl:Class>
	
	<owl:Class rdf:about="&fibo-be-oac-cpty;DeJureControllingInterest">
		<rdfs:subClassOf rdf:resource="&fibo-fnd-oac-ctl;DeJureControl"/>
		<rdfs:label>de jure controlling interest</rdfs:label>
		<skos:definition>controlling interest that is formalized by some formal legal construct</skos:definition>
	</owl:Class>
	
	<owl:Class rdf:about="&fibo-be-oac-cpty;DeJureControllingInterestParty">
		<rdfs:subClassOf rdf:resource="&fibo-be-oac-cpty;ControllingInterestParty"/>
		<rdfs:subClassOf>
			<owl:Restriction>
				<owl:onProperty rdf:resource="&fibo-be-oac-cpty;holdsSomeMeansOf"/>
				<owl:someValuesFrom rdf:resource="&fibo-be-oac-cpty;DeJureControllingInterest"/>
			</owl:Restriction>
		</rdfs:subClassOf>
		<rdfs:label>de jure controlling interest party</rdfs:label>
		<skos:definition>An entity that may exercise de jure controlling interest</skos:definition>
	</owl:Class>
	
	<owl:Class rdf:about="&fibo-be-oac-cpty;DegreeOfControl">
		<rdfs:subClassOf rdf:resource="&fibo-fnd-rel-rel;Reference"/>
		<rdfs:subClassOf>
			<owl:Restriction>
				<owl:onProperty rdf:resource="&fibo-be-oac-cpty;hasPercentageControl"/>
				<owl:someValuesFrom rdf:resource="&xsd;decimal"/>
			</owl:Restriction>
		</rdfs:subClassOf>
		<rdfs:label>degree of control</rdfs:label>
		<skos:definition>the degree of control one entity has over another</skos:definition>
	</owl:Class>
	
	<owl:Class rdf:about="&fibo-be-oac-cpty;EntityControllingParty">
		<rdfs:subClassOf rdf:resource="&fibo-fnd-oac-ctl;ControllingParty"/>
		<rdfs:subClassOf>
			<owl:Class>
				<owl:unionOf rdf:parseType="Collection">
					<owl:Restriction>
						<owl:onProperty rdf:resource="&fibo-fnd-rel-rel;controls"/>
						<owl:someValuesFrom rdf:resource="&fibo-be-le-lp;LegalEntity"/>
					</owl:Restriction>
					<owl:Restriction>
						<owl:onProperty rdf:resource="&fibo-be-oac-cpty;hasDegreeOfControl"/>
						<owl:allValuesFrom rdf:resource="&fibo-be-oac-cpty;DegreeOfControl"/>
					</owl:Restriction>
					<owl:Restriction>
						<owl:onProperty rdf:resource="&fibo-be-oac-cpty;hasNatureOfControl"/>
						<owl:allValuesFrom rdf:resource="&fibo-fnd-oac-ctl;DeFactoControl"/>
					</owl:Restriction>
				</owl:unionOf>
			</owl:Class>
		</rdfs:subClassOf>
		<rdfs:label>entity controlling party</rdfs:label>
		<skos:definition>Some party which is able to direct the activities of some business entity.</skos:definition>
		<skos:editorialNote>This type of party is either asserted to be the case by the entity itself or some other party, or is determined through some analysis or calculation based on the available information about controlling interests.</skos:editorialNote>
		<skos:scopeNote>It is assumed that since control follows from some form of ownership or contractual instrument, that the range of entities which may fulfil this party role is the same as that for entity ownership, namely a logical union of natural persons, legal persons and formal organizations.</skos:scopeNote>
	</owl:Class>
	
	<owl:Class rdf:about="&fibo-be-oac-cpty;EquityBasedDeJureControl">
		<rdfs:subClassOf rdf:resource="&fibo-be-oac-cpty;ConstitutionalDeJureControl"/>
		<rdfs:label>equity-based de jure control</rdfs:label>
		<skos:definition>De Jure controlling interest in an entity which is based on the holding of some form of equity in that entity.</skos:definition>
	</owl:Class>
	
	<owl:Class rdf:about="&fibo-be-oac-cpty;InfluenceBasedDeFactoControl">
		<rdfs:subClassOf rdf:resource="&fibo-fnd-oac-ctl;DeFactoControl"/>
		<rdfs:label>influence-based de facto control</rdfs:label>
		<skos:definition>Some influence and control over some entity other than by means of investment in that entity.</skos:definition>
	</owl:Class>
	
	<owl:Class rdf:about="&fibo-be-oac-cpty;InfluenceBasedDeFactoControllingParty">
		<rdfs:subClassOf rdf:resource="&fibo-be-oac-cpty;DeFactoControllingInterestParty"/>
		<rdfs:subClassOf>
			<owl:Restriction>
				<owl:onProperty rdf:resource="&fibo-fnd-pty-rl;isPlayedBy"/>
				<owl:someValuesFrom>
					<owl:Restriction>
						<owl:onProperty rdf:resource="&fibo-be-oac-cpty;holdsSomeMeansOf"/>
						<owl:allValuesFrom rdf:resource="&fibo-be-oac-cpty;InfluenceBasedDeFactoControl"/>
					</owl:Restriction>
				</owl:someValuesFrom>
			</owl:Restriction>
		</rdfs:subClassOf>
		<rdfs:label>influence-based de facto controlling party</rdfs:label>
		<skos:definition>A party which exercises some influence and control over the entity other than by means of investment.</skos:definition>
		<skos:editorialNote>Regulatory or jurisdictional control would fall under this control. Court appointed control is de jure control BUT the scenario in which a government takes over something and then hands it over to some new de jure controller i.e. administrator - in the meantime this is de facto control by e.g. the government.</skos:editorialNote>
	</owl:Class>
	
	<owl:Class rdf:about="&fibo-be-oac-cpty;InvestmentBasedDeFactoControl">
		<rdfs:subClassOf rdf:resource="&fibo-fnd-oac-ctl;DeFactoControl"/>
		<rdfs:label>investment-based de facto control</rdfs:label>
		<skos:definition>Control which arises through some investment in some entity, other than as the holding of constitutional equity (shares etc.) in that entity.</skos:definition>
	</owl:Class>
	
	<owl:Class rdf:about="&fibo-be-oac-cpty;InvestmentBasedDeFactoControllingInterestParty">
		<rdfs:subClassOf rdf:resource="&fibo-be-oac-cpty;DeFactoControllingInterestParty"/>
		<rdfs:subClassOf rdf:resource="&fibo-be-oac-opty;Investor"/>
		<rdfs:subClassOf>
			<owl:Restriction>
				<owl:onProperty rdf:resource="&fibo-be-oac-cpty;holdsSomeMeansOf"/>
				<owl:allValuesFrom rdf:resource="&fibo-be-oac-cpty;InvestmentBasedDeFactoControl"/>
			</owl:Restriction>
		</rdfs:subClassOf>
		<rdfs:label>investment-based de facto controlling interest party</rdfs:label>
		<skos:definition>A party which exercises some degree of de facto control based on some investment which they hold in the entity.</skos:definition>
	</owl:Class>
	
	<owl:Class rdf:about="&fibo-be-oac-cpty;JointControllingParty">
		<rdfs:subClassOf rdf:resource="&fibo-be-oac-cpty;EntityControllingParty"/>
		<rdfs:subClassOf>
			<owl:Restriction>
				<owl:onProperty rdf:resource="&fibo-fnd-rel-rel;hasIdentity"/>
				<owl:allValuesFrom rdf:resource="&fibo-be-oac-cpty;ControllingAlliance"/>
			</owl:Restriction>
		</rdfs:subClassOf>
		<rdfs:label>joint controlling party</rdfs:label>
		<owl:disjointWith rdf:resource="&fibo-be-oac-cpty;SoleControllingParty"/>
		<skos:definition>Some group of entities which collectively are able to direct the affairs of some business organization</skos:definition>
	</owl:Class>
	
	<owl:Class rdf:about="&fibo-be-oac-cpty;LimitedControllingParty">
		<rdfs:subClassOf rdf:resource="&fibo-be-oac-cpty;EntityControllingParty"/>
		<rdfs:subClassOf>
			<owl:Class>
				<owl:unionOf rdf:parseType="Collection">
					<owl:Restriction>
						<owl:onProperty rdf:resource="&fibo-fnd-rel-rel;controls"/>
						<owl:someValuesFrom rdf:resource="&fibo-be-le-lp;LegalEntity"/>
					</owl:Restriction>
					<owl:Restriction>
						<owl:onProperty rdf:resource="&fibo-be-oac-cpty;hasDegreeOfControl"/>
						<owl:allValuesFrom rdf:resource="&fibo-be-oac-cpty;DegreeOfControl"/>
					</owl:Restriction>
					<owl:Restriction>
						<owl:onProperty rdf:resource="&fibo-be-oac-cpty;hasNatureOfControl"/>
						<owl:allValuesFrom rdf:resource="&fibo-be-oac-cpty;LimitedDeFactoControl"/>
					</owl:Restriction>
				</owl:unionOf>
			</owl:Class>
		</rdfs:subClassOf>
		<rdfs:label>limited controlling party</rdfs:label>
		<skos:definition>Some individual entity which is able to direct the affairs of some business organization to a specific degree.</skos:definition>
		<skos:editorialNote>The degree to which the party has control of (is able to direct the activities of) the organization in question is defined as a percentage value where one hundred percent would equate to control without the involvement of others. The percentage of control is a calculated, determined or asserted value, and not necessarily a percentage of some controlling interest, though in the absence of other factors the determination of percentage of control would equate to the percentage of controlling interest e.g. voting shares held.</skos:editorialNote>
	</owl:Class>
	
	<owl:Class rdf:about="&fibo-be-oac-cpty;LimitedDeFactoControl">
		<rdfs:subClassOf rdf:resource="&fibo-fnd-oac-ctl;DeFactoControl"/>
		<rdfs:label>limited de facto control</rdfs:label>
		<skos:definition>The ability to direct the affairs of some entity within prescribed limits. Those limits are described in terms of activities which the entity holding such control may cause the controlled entity to carry out.</skos:definition>
	</owl:Class>
	
	<owl:Class rdf:about="&fibo-be-oac-cpty;MajorityControllingParty">
		<rdfs:subClassOf rdf:resource="&fibo-be-oac-cpty;EntityControllingParty"/>
		<rdfs:label>majority controlling party</rdfs:label>
		<skos:definition>an entity controlling party that possesses, either directly or indirectly, the power to direct or cause the direction of the management and policies of a legal person, whether through the ownership of a majority of voting securities, by contract, or otherwise</skos:definition>
		<fibo-fnd-utl-av:adaptedFrom>Electronic Code of Federal Regulations, Title 17, Chapter 1, Section 49.2</fibo-fnd-utl-av:adaptedFrom>
	</owl:Class>
	
	<owl:Class rdf:about="&fibo-be-oac-cpty;PartyHoldingSomeOptionForControl">
		<rdfs:subClassOf rdf:resource="&fibo-be-oac-cpty;ControllingInterestParty"/>
		<rdfs:subClassOf>
			<owl:Restriction>
				<owl:onProperty rdf:resource="&fibo-be-oac-cpty;holdsSomeMeansOf"/>
				<owl:someValuesFrom rdf:resource="&fibo-be-oac-cpty;DeJureControllingInterest"/>
			</owl:Restriction>
		</rdfs:subClassOf>
		<rdfs:label>party holding some option for control</rdfs:label>
		<skos:definition>Some party holding the option to exercise some de jure controlling interest</skos:definition>
		<skos:editorialNote>This will result in some potential change at a future time, in the conclusions about actual control.</skos:editorialNote>
	</owl:Class>
	
	<owl:Class rdf:about="&fibo-be-oac-cpty;Receiver">
		<rdfs:subClassOf rdf:resource="&fibo-be-oac-cpty;DeJureControllingInterestParty"/>
		<rdfs:subClassOf>
			<owl:Restriction>
				<owl:onProperty rdf:resource="&fibo-be-oac-cpty;holdsSomeMeansOf"/>
				<owl:someValuesFrom rdf:resource="&fibo-be-oac-cpty;CourtAppointedControl"/>
			</owl:Restriction>
		</rdfs:subClassOf>
		<rdfs:label>receiver</rdfs:label>
		<skos:definition>A party appointed by some court for the purposes of winding up the affairs of some entity which is no longer solvent.</skos:definition>
	</owl:Class>
	
	<owl:Class rdf:about="&fibo-be-oac-cpty;SignificantControllingInterestParty">
		<rdfs:subClassOf rdf:resource="&fibo-be-oac-cpty;DeJureControllingInterestParty"/>
		<rdfs:label>significant controlling interest party</rdfs:label>
		<skos:definition>A person which owns a significant voting stake in this entity of between some lower significant threshold and 50 percent, but not 50 percent or more.</skos:definition>
	</owl:Class>
	
	<owl:Class rdf:about="&fibo-be-oac-cpty;SoleControllingParty">
		<rdfs:subClassOf rdf:resource="&fibo-be-oac-cpty;EntityControllingParty"/>
		<rdfs:label>sole controlling party</rdfs:label>
		<skos:definition>an individual entity that directs the affairs of some formal business organization</skos:definition>
	</owl:Class>
	
	<owl:Class rdf:about="&fibo-be-oac-cpty;TotalOwner">
		<rdfs:subClassOf rdf:resource="&fibo-be-oac-opty;ConstitutionalOwner"/>
		<rdfs:label>total owner</rdfs:label>
		<skos:definition>Entity having 100 percent ownership in the entity so owned.</skos:definition>
		<skos:editorialNote>By virtue of holding 100 percent of the equity ownership, the Total Owner also holds 100 percent of the controlling equity, if there is a difference. Therefore it is both a total owner and a total controlling party.</skos:editorialNote>
	</owl:Class>
	
	<owl:Class rdf:about="&fibo-be-oac-cpty;WarrantHolder">
		<rdfs:subClassOf rdf:resource="&fibo-be-oac-cpty;PartyHoldingSomeOptionForControl"/>
		<rdfs:label>warrant holder</rdfs:label>
		<skos:definition>A holder of some warrant which when exercised would confer upon that party some de jure controlling interest in some entity.</skos:definition>
	</owl:Class>
	
	<owl:ObjectProperty rdf:about="&fibo-be-oac-cpty;hasControllingInterestParty">
		<rdfs:subPropertyOf rdf:resource="&fibo-fnd-pty-pty;hasPartyInRole"/>
		<rdfs:label>has controlling interest party</rdfs:label>
		<rdfs:domain rdf:resource="&fibo-be-le-lp;LegalEntity"/>
		<rdfs:range rdf:resource="&fibo-be-oac-cpty;ControllingInterestParty"/>
		<skos:definition>indicates an entity that has the ability to exercise some control over a formal business organization</skos:definition>
	</owl:ObjectProperty>
	
	<owl:ObjectProperty rdf:about="&fibo-be-oac-cpty;hasDegreeOfControl">
		<rdfs:subPropertyOf rdf:resource="&lcc-lr;has"/>
		<rdfs:label>has degree of control</rdfs:label>
		<rdfs:domain rdf:resource="&fibo-be-oac-cpty;EntityControllingParty"/>
		<rdfs:range rdf:resource="&fibo-be-oac-cpty;DegreeOfControl"/>
		<skos:definition>has degree of control, (partial, majority, or complete) either alone or with other parties, with respect to some activity</skos:definition>
	</owl:ObjectProperty>
	
	<owl:ObjectProperty rdf:about="&fibo-be-oac-cpty;hasMajorityControllingParty">
		<rdfs:subPropertyOf rdf:resource="&fibo-be-oac-cpty;isControlledToSomeDegreeBy"/>
		<rdfs:label>has majority controlling party</rdfs:label>
		<rdfs:domain rdf:resource="&fibo-be-le-lp;LegalEntity"/>
		<rdfs:range rdf:resource="&fibo-be-oac-cpty;MajorityControllingParty"/>
		<skos:definition>The parent of the company, if there is one.</skos:definition>
		<skos:editorialNote>This is usually (but not necessarily) any entity which owns a controlling stake (50 percent plus one voting share or above, or equivalent) in this company, if it is a limited company.</skos:editorialNote>
	</owl:ObjectProperty>
	
	<owl:ObjectProperty rdf:about="&fibo-be-oac-cpty;hasNatureOfControl">
		<rdfs:subPropertyOf rdf:resource="&lcc-lr;has"/>
		<rdfs:label>has nature of control</rdfs:label>
		<rdfs:domain rdf:resource="&fibo-be-oac-cpty;EntityControllingParty"/>
		<rdfs:range rdf:resource="&fibo-fnd-oac-ctl;DeFactoControl"/>
		<skos:definition>has nature or kind of control, de facto or limited de facto control</skos:definition>
	</owl:ObjectProperty>
	
	<owl:DatatypeProperty rdf:about="&fibo-be-oac-cpty;hasPercentageControl">
		<rdfs:label>has percentage control</rdfs:label>
		<rdfs:domain rdf:resource="&fibo-be-oac-cpty;DegreeOfControl"/>
		<rdfs:range rdf:resource="&xsd;decimal"/>
		<skos:definition>indicates the percentage (out of 100) control that one party has over another</skos:definition>
	</owl:DatatypeProperty>
	
	<owl:ObjectProperty rdf:about="&fibo-be-oac-cpty;hasSignificantControllingInterestParty">
		<rdfs:subPropertyOf rdf:resource="&fibo-be-oac-cpty;hasControllingInterestParty"/>
		<rdfs:label>has significant controlling interest party</rdfs:label>
		<rdfs:domain rdf:resource="&fibo-be-le-lp;LegalEntity"/>
		<rdfs:range rdf:resource="&fibo-be-oac-cpty;SignificantControllingInterestParty"/>
		<skos:definition>identifies an entity that owns a significant percentage of the equity in this company, but less than 50 percent</skos:definition>
		<skos:editorialNote>This is a relationship for any ownership between a lower threshold (defined in AML regulations locally) and 50 percent. It is the inverse of the Affiliate (AKA Associate) relationship.</skos:editorialNote>
	</owl:ObjectProperty>
	
	<owl:ObjectProperty rdf:about="&fibo-be-oac-cpty;hasTotalOwner">
		<rdfs:subPropertyOf rdf:resource="&fibo-be-oac-opty;hasConstitutionalOwner"/>
		<rdfs:label>has total owner</rdfs:label>
		<rdfs:domain rdf:resource="&fibo-be-le-lp;LegalEntity"/>
		<rdfs:range rdf:resource="&fibo-be-oac-cpty;TotalOwner"/>
		<skos:definition>indicates the party that wholly controls the organization, i.e., one that owns 100 percent interest</skos:definition>
		<skos:editorialNote>This may be any entity which is capable of exercising ownership. Scope Note: By virtue of holding 100 percent of the equity ownership, the Total Owner also holds 100 percent of the controlling equity, if there is a difference. Therefore it is both a total owner and a total controlling party. For this reason it is included among the control relationships and is a specialization of the has majority controlling party relationships.</skos:editorialNote>
	</owl:ObjectProperty>
	
	<owl:ObjectProperty rdf:about="&fibo-be-oac-cpty;holdsSomeMeansOf">
		<rdfs:label>holds some means of</rdfs:label>
		<rdfs:domain rdf:resource="&fibo-be-oac-cpty;ControllingInterestParty"/>
		<rdfs:range rdf:resource="&fibo-fnd-oac-ctl;ControllingCapacity"/>
		<skos:definition>Some means of control held by the party.</skos:definition>
	</owl:ObjectProperty>
	
	<owl:ObjectProperty rdf:about="&fibo-be-oac-cpty;isBasedOnInvestmentEquity">
		<rdfs:subPropertyOf rdf:resource="&fibo-fnd-rel-rel;isConferredBy"/>
		<rdfs:label>is based on investment equity</rdfs:label>
		<rdfs:domain rdf:resource="&fibo-be-oac-cpty;InvestmentBasedDeFactoControl"/>
		<rdfs:range rdf:resource="&fibo-be-oac-opty;InvestmentEquity"/>
		<skos:definition>indicates investment-based de facto control, which is is based on the holding of some investment equity by some party</skos:definition>
	</owl:ObjectProperty>
	
	<owl:ObjectProperty rdf:about="&fibo-be-oac-cpty;isControlledToSomeDegreeBy">
		<rdfs:subPropertyOf rdf:resource="&fibo-fnd-rel-rel;isControlledBy"/>
		<rdfs:label>is controlled to some degree by</rdfs:label>
		<rdfs:domain rdf:resource="&fibo-be-le-lp;LegalEntity"/>
		<rdfs:range rdf:resource="&fibo-be-oac-cpty;EntityControllingParty"/>
		<skos:definition>identifies a party that has some degree of control over a formal business organization</skos:definition>
		<skos:editorialNote>Control by this type of party is either asserted to be the case by the entity itself or some other party, or is determined through some analysis or calculation based on the available information about controlling interests.</skos:editorialNote>
	</owl:ObjectProperty>

</rdf:RDF>