<?xml version="1.0" encoding="UTF-8"?>
<!DOCTYPE rdf:RDF [
	<!ENTITY dct "http://purl.org/dc/terms/">
	<!ENTITY fibo-be-corp-corp "https://spec.edmcouncil.org/fibo/BE/Corporations/Corporations/">
	<!ENTITY fibo-be-le-cb "https://spec.edmcouncil.org/fibo/BE/LegalEntities/CorporateBodies/">
	<!ENTITY fibo-be-oac-cown "https://spec.edmcouncil.org/fibo/BE/OwnershipAndControl/CorporateOwnership/">
	<!ENTITY fibo-be-oac-opty "https://spec.edmcouncil.org/fibo/BE/OwnershipAndControl/OwnershipParties/">
	<!ENTITY fibo-fnd-aap-agt "https://spec.edmcouncil.org/fibo/FND/AgentsAndPeople/Agents/">
	<!ENTITY fibo-fnd-acc-aeq "https://spec.edmcouncil.org/fibo/FND/Accounting/AccountingEquity/">
	<!ENTITY fibo-fnd-agr-ctr "https://spec.edmcouncil.org/fibo/FND/Agreements/Contracts/">
	<!ENTITY fibo-fnd-pty-rl "https://spec.edmcouncil.org/fibo/FND/Parties/Roles/">
	<!ENTITY fibo-fnd-rel-rel "https://spec.edmcouncil.org/fibo/FND/Relations/Relations/">
	<!ENTITY fibo-fnd-utl-av "https://spec.edmcouncil.org/fibo/FND/Utilities/AnnotationVocabulary/">
	<!ENTITY owl "http://www.w3.org/2002/07/owl#">
	<!ENTITY rdf "http://www.w3.org/1999/02/22-rdf-syntax-ns#">
	<!ENTITY rdfs "http://www.w3.org/2000/01/rdf-schema#">
	<!ENTITY skos "http://www.w3.org/2004/02/skos/core#">
	<!ENTITY sm "http://www.omg.org/techprocess/ab/SpecificationMetadata/">
	<!ENTITY xsd "http://www.w3.org/2001/XMLSchema#">
]>
<rdf:RDF
	xml:base="https://spec.edmcouncil.org/fibo/BE/OwnershipAndControl/CorporateOwnership/"
	xmlns:dct="http://purl.org/dc/terms/"
	xmlns:fibo-be-corp-corp="https://spec.edmcouncil.org/fibo/BE/Corporations/Corporations/"
	xmlns:fibo-be-le-cb="https://spec.edmcouncil.org/fibo/BE/LegalEntities/CorporateBodies/"
	xmlns:fibo-be-oac-cown="https://spec.edmcouncil.org/fibo/BE/OwnershipAndControl/CorporateOwnership/"
	xmlns:fibo-be-oac-opty="https://spec.edmcouncil.org/fibo/BE/OwnershipAndControl/OwnershipParties/"
	xmlns:fibo-fnd-aap-agt="https://spec.edmcouncil.org/fibo/FND/AgentsAndPeople/Agents/"
	xmlns:fibo-fnd-acc-aeq="https://spec.edmcouncil.org/fibo/FND/Accounting/AccountingEquity/"
	xmlns:fibo-fnd-agr-ctr="https://spec.edmcouncil.org/fibo/FND/Agreements/Contracts/"
	xmlns:fibo-fnd-pty-rl="https://spec.edmcouncil.org/fibo/FND/Parties/Roles/"
	xmlns:fibo-fnd-rel-rel="https://spec.edmcouncil.org/fibo/FND/Relations/Relations/"
	xmlns:fibo-fnd-utl-av="https://spec.edmcouncil.org/fibo/FND/Utilities/AnnotationVocabulary/"
	xmlns:owl="http://www.w3.org/2002/07/owl#"
	xmlns:rdf="http://www.w3.org/1999/02/22-rdf-syntax-ns#"
	xmlns:rdfs="http://www.w3.org/2000/01/rdf-schema#"
	xmlns:skos="http://www.w3.org/2004/02/skos/core#"
	xmlns:sm="http://www.omg.org/techprocess/ab/SpecificationMetadata/"
	xmlns:xsd="http://www.w3.org/2001/XMLSchema#">
	
	<owl:Ontology
		rdf:about="https://spec.edmcouncil.org/fibo/BE/OwnershipAndControl/CorporateOwnership/">
		<rdfs:label>Corporate Ownership Ontology</rdfs:label>
		<dct:license
			rdf:datatype="&xsd;anyURI">http://www.omg.org/techprocess/ab/SpecificationMetadata/MITLicense</dct:license>
		<sm:contentLanguage
			rdf:datatype="&xsd;anyURI">http://www.omg.org/spec/ODM/</sm:contentLanguage>
		<sm:contentLanguage
			rdf:datatype="&xsd;anyURI">http://www.w3.org/standards/techs/owl#w3c_all</sm:contentLanguage>
		<sm:copyright>Copyright (c) 2013-2016 EDM Council, Inc.
Copyright (c) 2013-2016 Object Management Group, Inc.</sm:copyright>
		<sm:dependsOn
			rdf:datatype="&xsd;anyURI">https://spec.edmcouncil.org/fibo/BE/Corporations/Corporations/</sm:dependsOn>
		<sm:dependsOn
			rdf:datatype="&xsd;anyURI">https://spec.edmcouncil.org/fibo/BE/OwnershipAndControl/OwnershipParties/</sm:dependsOn>
		<sm:dependsOn
			rdf:datatype="&xsd;anyURI">https://spec.edmcouncil.org/fibo/FND/</sm:dependsOn>
		<sm:fileAbbreviation>fibo-be-oac-cown</sm:fileAbbreviation>
		<sm:fileAbstract>This ontology defines concepts relating to corporation-specific ownership. Roles are defined in terms of the ownership enjoyed by the party, and are the specific examples of these concepts as they apply to companies incorporated by the issuance of shares.</sm:fileAbstract>
		<sm:filename>CorporateOwnership.rdf</sm:filename>
		<rdfs:seeAlso
			rdf:datatype="&xsd;anyURI">https://spec.edmcouncil.org/fibo/AboutTheEDMC-FIBOFamily/</rdfs:seeAlso>
		<rdfs:seeAlso
			rdf:datatype="&xsd;anyURI">https://spec.edmcouncil.org/fibo/BE/AboutBE/</rdfs:seeAlso>
		<rdfs:seeAlso
			rdf:datatype="&xsd;anyURI">https://spec.edmcouncil.org/fibo/BE/OwnershipAndControl/AboutBEOwnershipAndControl/</rdfs:seeAlso>
		<owl:imports
			rdf:resource="https://spec.edmcouncil.org/fibo/BE/Corporations/Corporations/"/>
		<owl:imports
			rdf:resource="https://spec.edmcouncil.org/fibo/BE/LegalEntities/CorporateBodies/"/>
		<owl:imports
			rdf:resource="https://spec.edmcouncil.org/fibo/BE/OwnershipAndControl/OwnershipParties/"/>
		<owl:imports
			rdf:resource="https://spec.edmcouncil.org/fibo/FND/Accounting/AccountingEquity/"/>
		<owl:imports
			rdf:resource="https://spec.edmcouncil.org/fibo/FND/AgentsAndPeople/Agents/"/>
		<owl:imports
			rdf:resource="https://spec.edmcouncil.org/fibo/FND/Agreements/Contracts/"/>
		<owl:imports
			rdf:resource="https://spec.edmcouncil.org/fibo/FND/Parties/Roles/"/>
		<owl:imports
			rdf:resource="https://spec.edmcouncil.org/fibo/FND/Relations/Relations/"/>
		<owl:imports
			rdf:resource="https://spec.edmcouncil.org/fibo/FND/Utilities/AnnotationVocabulary/"/>
		<owl:versionIRI
			rdf:resource="https://spec.edmcouncil.org/fibo/BE/20160201/OwnershipAndControl/CorporateOwnership/"/>
		<skos:changeNote>The https://spec.edmcouncil.org/fibo/BE/20131101/OwnershipAndControl/CorporateOwnership.rdf version of this ontology was modified per the issue resolutions identified in the FIBO BE 1.0 FTF report.</skos:changeNote>
	</owl:Ontology>
	
	<owl:Class
		rdf:about="&fibo-be-oac-cown;BeneficialOwner">
		<rdfs:subClassOf
			rdf:resource="&fibo-be-oac-cown;Shareholder"/>
		<rdfs:label>beneficial owner</rdfs:label>
		<skos:definition>Entity that enjoys the possession and/or benefits of ownership (such as receipt of income) of a property even though its ownership (title) is in the name of another entity (called a nominee or registered owner). Use of a nominee (who may be an agent, custodian, or a trustee) does not change the position regarding tax reporting and tax liability, and the beneficial-owner remains responsible.</skos:definition>
		<skos:editorialNote>This covers entities which have any kind of control. From World Bank Report: In identifying the beneficial owner, the focus should be on two factors: the control exercised and the benefit derived. Control of a corporate vehicle will always depend on context, as control can be exercised in many different ways, including through ownership, contractually or informally.</skos:editorialNote>
		<fibo-fnd-utl-av:definitionOrigin
			rdf:datatype="&xsd;anyURI">http://www.businessdictionary.com/definition/beneficial-owner.html</fibo-fnd-utl-av:definitionOrigin>
		<fibo-fnd-utl-av:synonym>actual owner</fibo-fnd-utl-av:synonym>
	</owl:Class>
	
	<owl:Class
		rdf:about="&fibo-be-oac-cown;PublicShareholder">
		<rdfs:subClassOf
			rdf:resource="&fibo-be-oac-cown;Shareholder"/>
		<rdfs:label>public shareholder</rdfs:label>
		<skos:definition>a shareholder that holds publicly issued shares in a listed company</skos:definition>
	</owl:Class>
	
	<owl:Class
		rdf:about="&fibo-be-oac-cown;RegisteredShareholder">
		<rdfs:subClassOf
			rdf:resource="&fibo-be-oac-cown;Shareholder"/>
		<rdfs:label>registered shareholder</rdfs:label>
		<skos:definition>a shareholder that is registered on the shareholder registry for a company</skos:definition>
	</owl:Class>
	
	<owl:Class
		rdf:about="&fibo-be-oac-cown;Shareholder">
		<rdfs:subClassOf
			rdf:resource="&fibo-be-oac-opty;ConstitutionalOwner"/>
		<rdfs:subClassOf
			rdf:resource="&fibo-fnd-agr-ctr;TransferableContractHolder"/>
		<rdfs:subClassOf>
			<owl:Restriction>
				<owl:onProperty
					rdf:resource="&fibo-fnd-pty-rl;isPlayedBy"/>
				<owl:someValuesFrom>
					<owl:Restriction>
						<owl:allValuesFrom
							rdf:resource="&fibo-fnd-acc-aeq;StockholdersEquity"/>
						<owl:onProperty
							rdf:resource="&fibo-be-oac-opty;holdsEquityIn"/>
					</owl:Restriction>
				</owl:someValuesFrom>
			</owl:Restriction>
		</rdfs:subClassOf>
		<rdfs:label>shareholder</rdfs:label>
		<skos:definition>An individual, group, or organization that owns one or more shares in a company, and in whose name the share certificate is issued.  It is legal for a company to have only one shareholder. Also called (in the US) stockholder.</skos:definition>
		<fibo-fnd-utl-av:definitionOrigin
			rdf:datatype="&xsd;anyURI">http://www.businessdictionary.com/definition/shareholder.html</fibo-fnd-utl-av:definitionOrigin>
	</owl:Class>
	
	<owl:Class
		rdf:about="&fibo-be-oac-cown;Shareholding">
		<rdfs:subClassOf
			rdf:resource="&fibo-fnd-acc-aeq;FinancialAsset"/>
		<rdfs:subClassOf>
			<owl:Restriction>
				<owl:allValuesFrom
					rdf:resource="&fibo-be-oac-cown;Shareholder"/>
				<owl:onProperty
					rdf:resource="&fibo-be-oac-opty;isEquityHeldBy"/>
			</owl:Restriction>
		</rdfs:subClassOf>
		<rdfs:label>shareholding</rdfs:label>
		<skos:definition>Legal power of stockholders (shareholders) varies in proportion to their shareholdings. Typically, ten percent and below stockholding provides no protection. Fifteen percent stockholding may give the power to petition courts against changing the shares class rights. Up to 49.9 percent stockholding normally gives power to demand calling of an extraordinary general meeting. Fifty percent and over stockholding gives power to fire a director and force out minority stockholders by acquiring their shares as per the rules of the firm. Holder of 75 percent of the stock has the power to change the articles and memorandum of association and the firms name, reduce the share capital, allow the firm to buy its own shares from other stockholders, and to shut down the business. One hundred percent stockholding of course gives total power under the corporate legislation.</skos:definition>
		<fibo-fnd-utl-av:definitionOrigin
			rdf:datatype="&xsd;anyURI">http://www.businessdictionary.com/definition/company-shareholdings.html</fibo-fnd-utl-av:definitionOrigin>
	</owl:Class>
	
	<owl:ObjectProperty
		rdf:about="&fibo-be-oac-cown;shareholderHoldsEquity">
		<rdfs:label>shareholder holds equity</rdfs:label>
	</owl:ObjectProperty>

</rdf:RDF>