<?xml version="1.0" encoding="UTF-8"?>
<!DOCTYPE rdf:RDF [
	<!ENTITY dct "http://purl.org/dc/terms/">
	<!ENTITY fibo-fnd-aap-agt "https://spec.edmcouncil.org/fibo/FND/AgentsAndPeople/Agents/">
	<!ENTITY fibo-fnd-acc-cur "https://spec.edmcouncil.org/fibo/FND/Accounting/CurrencyAmount/">
	<!ENTITY fibo-fnd-dt-fd "https://spec.edmcouncil.org/fibo/FND/DatesAndTimes/FinancialDates/">
	<!ENTITY fibo-fnd-rel-rel "https://spec.edmcouncil.org/fibo/FND/Relations/Relations/">
	<!ENTITY fibo-fnd-utl-av "https://spec.edmcouncil.org/fibo/FND/Utilities/AnnotationVocabulary/">
	<!ENTITY fibo-ind-ind-ind "https://spec.edmcouncil.org/fibo/IND/Indicators/Indicators/">
	<!ENTITY fibo-ind-ir-ir "https://spec.edmcouncil.org/fibo/IND/InterestRates/InterestRates/">
	<!ENTITY owl "http://www.w3.org/2002/07/owl#">
	<!ENTITY rdf "http://www.w3.org/1999/02/22-rdf-syntax-ns#">
	<!ENTITY rdfs "http://www.w3.org/2000/01/rdf-schema#">
	<!ENTITY skos "http://www.w3.org/2004/02/skos/core#">
	<!ENTITY sm "http://www.omg.org/techprocess/ab/SpecificationMetadata/">
	<!ENTITY xsd "http://www.w3.org/2001/XMLSchema#">
]>
<rdf:RDF
	xml:base="https://spec.edmcouncil.org/fibo/IND/InterestRates/InterestRates/"
	xmlns:dct="http://purl.org/dc/terms/"
	xmlns:fibo-fnd-aap-agt="https://spec.edmcouncil.org/fibo/FND/AgentsAndPeople/Agents/"
	xmlns:fibo-fnd-acc-cur="https://spec.edmcouncil.org/fibo/FND/Accounting/CurrencyAmount/"
	xmlns:fibo-fnd-dt-fd="https://spec.edmcouncil.org/fibo/FND/DatesAndTimes/FinancialDates/"
	xmlns:fibo-fnd-rel-rel="https://spec.edmcouncil.org/fibo/FND/Relations/Relations/"
	xmlns:fibo-fnd-utl-av="https://spec.edmcouncil.org/fibo/FND/Utilities/AnnotationVocabulary/"
	xmlns:fibo-ind-ind-ind="https://spec.edmcouncil.org/fibo/IND/Indicators/Indicators/"
	xmlns:fibo-ind-ir-ir="https://spec.edmcouncil.org/fibo/IND/InterestRates/InterestRates/"
	xmlns:owl="http://www.w3.org/2002/07/owl#"
	xmlns:rdf="http://www.w3.org/1999/02/22-rdf-syntax-ns#"
	xmlns:rdfs="http://www.w3.org/2000/01/rdf-schema#"
	xmlns:skos="http://www.w3.org/2004/02/skos/core#"
	xmlns:sm="http://www.omg.org/techprocess/ab/SpecificationMetadata/"
	xmlns:xsd="http://www.w3.org/2001/XMLSchema#">
	
	<owl:Ontology
		rdf:about="https://spec.edmcouncil.org/fibo/IND/InterestRates/InterestRates/">
		<rdfs:label>Interest Rates Ontology</rdfs:label>
		<dct:license
			rdf:resource="&sm;MITLicense"/>
		<sm:contentLanguage
			rdf:resource="http://www.omg.org/spec/ODM/"/>
		<sm:contentLanguage
			rdf:resource="http://www.w3.org/standards/techs/owl#w3c_all"/>
		<sm:copyright>Copyright (c) 2014-2017 EDM Council, Inc.
Copyright (c) 2014-2017 Object Management Group, Inc.</sm:copyright>
		<sm:dependsOn
			rdf:resource="https://spec.edmcouncil.org/fibo/FND/"/>
		<sm:dependsOn
			rdf:resource="https://spec.edmcouncil.org/fibo/IND/Indicators/Indicators/"/>
		<sm:fileAbbreviation>fibo-ind-ir-ir</sm:fileAbbreviation>
		<sm:fileAbstract>This ontology provides the basic types of interest rate which are recognized in the financial markets, and the relationships between these where applicable. These include bank base rates, inter-bank offer rates, overnight rates of interest and the US Federal Funds rate which is widely used as a rate of reference. It also includes the concept of a market rate spread between two interest rates.</sm:fileAbstract>
		<sm:filename>InterestRates.rdf</sm:filename>
		<rdfs:seeAlso
			rdf:resource="https://spec.edmcouncil.org/fibo/AboutTheEDMC-FIBOFamily/"/>
		<rdfs:seeAlso
			rdf:resource="https://spec.edmcouncil.org/fibo/IND/AboutIND/"/>
		<rdfs:seeAlso
			rdf:resource="https://spec.edmcouncil.org/fibo/IND/InterestRates/AboutInterestRates/"/>
		<owl:imports
			rdf:resource="https://spec.edmcouncil.org/fibo/FND/Accounting/CurrencyAmount/"/>
		<owl:imports
			rdf:resource="https://spec.edmcouncil.org/fibo/FND/AgentsAndPeople/Agents/"/>
		<owl:imports
			rdf:resource="https://spec.edmcouncil.org/fibo/FND/DatesAndTimes/FinancialDates/"/>
		<owl:imports
			rdf:resource="https://spec.edmcouncil.org/fibo/FND/Relations/Relations/"/>
		<owl:imports
			rdf:resource="https://spec.edmcouncil.org/fibo/FND/Utilities/AnnotationVocabulary/"/>
		<owl:imports
			rdf:resource="https://spec.edmcouncil.org/fibo/IND/Indicators/Indicators/"/>
		<owl:versionIRI
			rdf:resource="https://spec.edmcouncil.org/fibo/IND/20170201/InterestRates/InterestRates/"/>
		<skos:changeNote>The https://spec.edmcouncil.org/fibo/IND/20140601/InterestRates/InterestRates.rdf version of this ontology was modified per the issue resolutions identified in the FIBO IND 1.0 FTF 1 report.</skos:changeNote>
		<skos:changeNote>The https://spec.edmcouncil.org/fibo/IND/20150501/InterestRates/InterestRates.rdf version of this ontology was modified per the issue resolutions identified in the FIBO IND 1.0 FTF 2 report.</skos:changeNote>
		<skos:changeNote>The https://spec.edmcouncil.org/fibo/IND/20160801/InterestRates/InterestRates.rdf version of this ontology was modified per the issue resolutions identified in the FIBO IND 1.1 RTF report.</skos:changeNote>
	</owl:Ontology>
	
	<owl:Class
		rdf:about="&fibo-ind-ir-ir;BaseRate">
		<rdfs:subClassOf
			rdf:resource="&fibo-ind-ir-ir;ReferenceInterestRate"/>
		<rdfs:label>base rate</rdfs:label>
		<skos:definition>a reference rate that is the base rate set by a central bank for a given currency</skos:definition>
		<fibo-fnd-utl-av:explanatoryNote>This is set at intervals.</fibo-fnd-utl-av:explanatoryNote>
	</owl:Class>
	
	<fibo-fnd-dt-fd:ExplicitDuration
		rdf:about="&fibo-ind-ir-ir;EighteenMonths">
		<rdf:type
			rdf:resource="&owl;NamedIndividual"/>
		<rdfs:label>eighteen months</rdfs:label>
		<skos:definition>a duration of exactly eighteen (18) months, regardless of the length in days of a given calendar month, but typically 30 days</skos:definition>
		<fibo-fnd-dt-fd:hasDurationValue>P18M</fibo-fnd-dt-fd:hasDurationValue>
	</fibo-fnd-dt-fd:ExplicitDuration>
	
	<owl:Class
		rdf:about="&fibo-ind-ir-ir;FederalFundsRate">
		<rdfs:subClassOf
			rdf:resource="&fibo-ind-ir-ir;OvernightRate"/>
		<rdfs:label>federal funds rate</rdfs:label>
		<rdfs:seeAlso
			rdf:resource="http://www.newyorkfed.org/markets/omo/dmm/fedfundsdata.cfm"/>
		<skos:altLabel>fed funds rate</skos:altLabel>
		<skos:definition>a reference rate that is the interest rate at which a depository institution lends funds maintained at the Federal Reserve to another depository institution overnight</skos:definition>
		<skos:prefLabel>US federal funds rate</skos:prefLabel>
		<fibo-fnd-utl-av:explanatoryNote>By trading government securities, the New York Fed affects the federal funds rate, which is the interest rate at which depository institutions lend balances to each other overnight. The Federal Open Market Committee establishes the target rate for trading in the federal funds market.</fibo-fnd-utl-av:explanatoryNote>
		<fibo-fnd-utl-av:explanatoryNote>The federal funds rate is generally only applicable to the most creditworthy institutions when they borrow and lend overnight funds to each other. The federal funds rate is one of the most influential interest rates in the U.S. economy, since it affects monetary and financial conditions, which in turn have a bearing on key aspects of the broad economy including employment, growth and inflation. The Federal Open Market Committee (FOMC), which is the Federal Reserve&apos;s primary monetary policymaking body, telegraphs its desired target for the federal funds rate through open market operations.</fibo-fnd-utl-av:explanatoryNote>
	</owl:Class>
	
	<fibo-fnd-dt-fd:ExplicitDuration
		rdf:about="&fibo-ind-ir-ir;FifteenYears">
		<rdf:type
			rdf:resource="&owl;NamedIndividual"/>
		<rdfs:label>fifteen years</rdfs:label>
		<skos:definition>a duration of exactly fifteen (15) years</skos:definition>
		<fibo-fnd-dt-fd:hasDurationValue>P15Y</fibo-fnd-dt-fd:hasDurationValue>
	</fibo-fnd-dt-fd:ExplicitDuration>
	
	<fibo-fnd-dt-fd:ExplicitDuration
		rdf:about="&fibo-ind-ir-ir;FiveYears">
		<rdf:type
			rdf:resource="&owl;NamedIndividual"/>
		<rdfs:label>five years</rdfs:label>
		<skos:definition>a duration of exactly five (5) years</skos:definition>
		<fibo-fnd-dt-fd:hasDurationValue>P5Y</fibo-fnd-dt-fd:hasDurationValue>
	</fibo-fnd-dt-fd:ExplicitDuration>
	
	<fibo-fnd-dt-fd:ExplicitDuration
		rdf:about="&fibo-ind-ir-ir;FortyEightMonths">
		<rdf:type
			rdf:resource="&owl;NamedIndividual"/>
		<rdfs:label>forty-eight months</rdfs:label>
		<skos:definition>a duration of exactly forty-eight (48) months, regardless of the length in days of a given calendar month, but typically 30 days</skos:definition>
		<fibo-fnd-dt-fd:hasDurationValue>P48M</fibo-fnd-dt-fd:hasDurationValue>
	</fibo-fnd-dt-fd:ExplicitDuration>
	
	<fibo-fnd-dt-fd:ExplicitDuration
		rdf:about="&fibo-ind-ir-ir;FourYears">
		<rdf:type
			rdf:resource="&owl;NamedIndividual"/>
		<rdfs:label>four years</rdfs:label>
		<skos:definition>a duration of exactly four (4) years</skos:definition>
		<fibo-fnd-dt-fd:hasDurationValue>P4Y</fibo-fnd-dt-fd:hasDurationValue>
	</fibo-fnd-dt-fd:ExplicitDuration>
	
	<owl:Class
		rdf:about="&fibo-ind-ir-ir;InterbankBidRate">
		<rdfs:subClassOf
			rdf:resource="&fibo-ind-ir-ir;InterbankRate"/>
		<rdfs:label>interbank bid rate</rdfs:label>
		<skos:definition>an interbank rate that is the interest rate at which participating banks are willing to borrow deposits from other banks</skos:definition>
		<fibo-fnd-utl-av:explanatoryNote>Unlike an interbank offered rate, which is the rate at which banks lend money, an interbank bid rate is the rate at which banks ask to borrow.</fibo-fnd-utl-av:explanatoryNote>
	</owl:Class>
	
	<owl:Class
		rdf:about="&fibo-ind-ir-ir;InterbankMidRate">
		<rdfs:subClassOf
			rdf:resource="&fibo-ind-ir-ir;InterbankRate"/>
		<rdfs:label>interbank mid rate</rdfs:label>
		<skos:definition>an interbank rate that represents the mid-point between bid and offer rates</skos:definition>
	</owl:Class>
	
	<owl:Class
		rdf:about="&fibo-ind-ir-ir;InterbankOfferedRate">
		<rdfs:subClassOf
			rdf:resource="&fibo-ind-ir-ir;InterbankRate"/>
		<rdfs:label>interbank offered rate</rdfs:label>
		<skos:definition>an interbank rate that is the interest rate at which participating banks lend money</skos:definition>
	</owl:Class>
	
	<owl:Class
		rdf:about="&fibo-ind-ir-ir;InterbankRate">
		<rdfs:subClassOf
			rdf:resource="&fibo-ind-ir-ir;ReferenceInterestRate"/>
		<rdfs:label>interbank rate</rdfs:label>
		<skos:definition>a reference rate that is the rate of interest charged on short-term loans between banks</skos:definition>
		<fibo-fnd-utl-av:explanatoryNote>Banks borrow and lend money in the interbank market in order to manage liquidity and meet the requirements placed on them. The interest rate charged depends on the availability of money in the market, on prevailing rates and on the specific terms of the contract, such as term length.</fibo-fnd-utl-av:explanatoryNote>
	</owl:Class>
	
	<fibo-fnd-dt-fd:ExplicitDuration
		rdf:about="&fibo-ind-ir-ir;NineMonths">
		<rdf:type
			rdf:resource="&owl;NamedIndividual"/>
		<rdfs:label>nine months</rdfs:label>
		<skos:definition>a duration of exactly nine (9) months, regardless of the length in days of a given calendar month, but typically 30 days</skos:definition>
		<fibo-fnd-dt-fd:hasDurationValue>P9M</fibo-fnd-dt-fd:hasDurationValue>
	</fibo-fnd-dt-fd:ExplicitDuration>
	
	<fibo-fnd-dt-fd:ExplicitDuration
		rdf:about="&fibo-ind-ir-ir;OneDay">
		<rdf:type
			rdf:resource="&owl;NamedIndividual"/>
		<rdfs:label>one day</rdfs:label>
		<skos:definition>a duration of exactly one day, or 24 hours, such as for an overnight rate</skos:definition>
		<fibo-fnd-dt-fd:hasDurationValue>P1D</fibo-fnd-dt-fd:hasDurationValue>
	</fibo-fnd-dt-fd:ExplicitDuration>
	
	<fibo-fnd-dt-fd:ExplicitDuration
		rdf:about="&fibo-ind-ir-ir;OneMonth">
		<rdf:type
			rdf:resource="&owl;NamedIndividual"/>
		<rdfs:label>one month</rdfs:label>
		<skos:definition>a duration of exactly one (1) month, regardless of the length in days of a given calendar month, but typically 30 days</skos:definition>
		<fibo-fnd-dt-fd:hasDurationValue>P1M</fibo-fnd-dt-fd:hasDurationValue>
	</fibo-fnd-dt-fd:ExplicitDuration>
	
	<fibo-fnd-dt-fd:ExplicitDuration
		rdf:about="&fibo-ind-ir-ir;OneWeek">
		<rdf:type
			rdf:resource="&owl;NamedIndividual"/>
		<rdfs:label>one week</rdfs:label>
		<skos:definition>a duration of exactly one week, or 7 days</skos:definition>
		<fibo-fnd-dt-fd:hasDurationValue>P7D</fibo-fnd-dt-fd:hasDurationValue>
	</fibo-fnd-dt-fd:ExplicitDuration>
	
	<fibo-fnd-dt-fd:ExplicitDuration
		rdf:about="&fibo-ind-ir-ir;OneYear">
		<rdf:type
			rdf:resource="&owl;NamedIndividual"/>
		<rdfs:label>one year</rdfs:label>
		<skos:definition>a duration of exactly one (1) year</skos:definition>
		<fibo-fnd-dt-fd:hasDurationValue>P1Y</fibo-fnd-dt-fd:hasDurationValue>
	</fibo-fnd-dt-fd:ExplicitDuration>
	
	<owl:Class
		rdf:about="&fibo-ind-ir-ir;OvernightRate">
		<rdfs:subClassOf
			rdf:resource="&fibo-ind-ir-ir;ReferenceInterestRate"/>
		<rdfs:subClassOf>
			<owl:Restriction>
				<owl:hasValue
					rdf:resource="&fibo-ind-ir-ir;OneDay"/>
				<owl:onProperty
					rdf:resource="&fibo-ind-ir-ir;hasTenor"/>
			</owl:Restriction>
		</rdfs:subClassOf>
		<rdfs:label>overnight rate</rdfs:label>
		<skos:definition>a reference rate that is an interest rate at which a depository institution lends funds to another depository institution (short-term), or the interest rate the central bank charges a financial institution to borrow money overnight</skos:definition>
		<fibo-fnd-utl-av:explanatoryNote>The overnight rate is the lowest available interest rate, and as such, it is only available to the most creditworthy institutions. It is the underlying rate for Overnight Interest Rate Swaps (IOS).</fibo-fnd-utl-av:explanatoryNote>
	</owl:Class>
	
	<owl:Class
		rdf:about="&fibo-ind-ir-ir;ReferenceInterestRate">
		<rdfs:subClassOf
			rdf:resource="&fibo-fnd-acc-cur;InterestRate"/>
		<rdfs:subClassOf
			rdf:resource="&fibo-ind-ind-ind;MarketRate"/>
		<rdfs:subClassOf>
			<owl:Restriction>
				<owl:allValuesFrom
					rdf:resource="&fibo-fnd-acc-cur;Currency"/>
				<owl:onProperty
					rdf:resource="&fibo-ind-ir-ir;hasReferenceCurrency"/>
			</owl:Restriction>
		</rdfs:subClassOf>
		<rdfs:subClassOf>
			<owl:Restriction>
				<owl:allValuesFrom
					rdf:resource="&fibo-fnd-dt-fd;Duration"/>
				<owl:onProperty
					rdf:resource="&fibo-ind-ir-ir;hasTenor"/>
			</owl:Restriction>
		</rdfs:subClassOf>
		<rdfs:label>reference interest rate</rdfs:label>
		<skos:definition>a market rate that is a rate of interest paid by or agreed among some bank or set of banks</skos:definition>
		<fibo-fnd-utl-av:explanatoryNote>The reference rate is a moving index such as LIBOR, the prime rate or the rate on benchmark U.S. Treasuries.</fibo-fnd-utl-av:explanatoryNote>
	</owl:Class>
	
	<fibo-fnd-dt-fd:ExplicitDuration
		rdf:about="&fibo-ind-ir-ir;SixMonths">
		<rdf:type
			rdf:resource="&owl;NamedIndividual"/>
		<rdfs:label>six months</rdfs:label>
		<skos:definition>a duration of exactly six (6) months, regardless of the length in days of a given calendar month, but typically 30 days</skos:definition>
		<fibo-fnd-dt-fd:hasDurationValue>P6M</fibo-fnd-dt-fd:hasDurationValue>
	</fibo-fnd-dt-fd:ExplicitDuration>
	
	<fibo-fnd-dt-fd:ExplicitDuration
		rdf:about="&fibo-ind-ir-ir;SixtyMonths">
		<rdf:type
			rdf:resource="&owl;NamedIndividual"/>
		<rdfs:label>sixty months</rdfs:label>
		<skos:definition>a duration of exactly sixty (60) months, regardless of the length in days of a given calendar month, but typically 30 days</skos:definition>
		<fibo-fnd-dt-fd:hasDurationValue>P60M</fibo-fnd-dt-fd:hasDurationValue>
	</fibo-fnd-dt-fd:ExplicitDuration>
	
	<fibo-fnd-dt-fd:ExplicitDuration
		rdf:about="&fibo-ind-ir-ir;TenYears">
		<rdf:type
			rdf:resource="&owl;NamedIndividual"/>
		<rdfs:label>ten years</rdfs:label>
		<skos:definition>a duration of exactly ten (10) years</skos:definition>
		<fibo-fnd-dt-fd:hasDurationValue>P10Y</fibo-fnd-dt-fd:hasDurationValue>
	</fibo-fnd-dt-fd:ExplicitDuration>
	
	<fibo-fnd-dt-fd:ExplicitDuration
		rdf:about="&fibo-ind-ir-ir;ThirtySixMonths">
		<rdf:type
			rdf:resource="&owl;NamedIndividual"/>
		<rdfs:label>thirty-six months</rdfs:label>
		<skos:definition>a duration of exactly thirty-six (36) months, regardless of the length in days of a given calendar month, but typically 30 days</skos:definition>
		<fibo-fnd-dt-fd:hasDurationValue>P36M</fibo-fnd-dt-fd:hasDurationValue>
	</fibo-fnd-dt-fd:ExplicitDuration>
	
	<fibo-fnd-dt-fd:ExplicitDuration
		rdf:about="&fibo-ind-ir-ir;ThirtyYears">
		<rdf:type
			rdf:resource="&owl;NamedIndividual"/>
		<rdfs:label>thirty years</rdfs:label>
		<skos:definition>a duration of exactly thirty (30) years</skos:definition>
		<fibo-fnd-dt-fd:hasDurationValue>P30Y</fibo-fnd-dt-fd:hasDurationValue>
	</fibo-fnd-dt-fd:ExplicitDuration>
	
	<fibo-fnd-dt-fd:ExplicitDuration
		rdf:about="&fibo-ind-ir-ir;ThreeMonths">
		<rdf:type
			rdf:resource="&owl;NamedIndividual"/>
		<rdfs:label>three months</rdfs:label>
		<skos:definition>a duration of exactly three (3) months, regardless of the length in days of a given calendar month, but typically 30 days</skos:definition>
		<fibo-fnd-dt-fd:hasDurationValue>P3M</fibo-fnd-dt-fd:hasDurationValue>
	</fibo-fnd-dt-fd:ExplicitDuration>
	
	<fibo-fnd-dt-fd:ExplicitDuration
		rdf:about="&fibo-ind-ir-ir;ThreeYears">
		<rdf:type
			rdf:resource="&owl;NamedIndividual"/>
		<rdfs:label>three years</rdfs:label>
		<skos:definition>a duration of exactly three (3) years</skos:definition>
		<fibo-fnd-dt-fd:hasDurationValue>P3Y</fibo-fnd-dt-fd:hasDurationValue>
	</fibo-fnd-dt-fd:ExplicitDuration>
	
	<fibo-fnd-dt-fd:ExplicitDuration
		rdf:about="&fibo-ind-ir-ir;TwelveMonths">
		<rdf:type
			rdf:resource="&owl;NamedIndividual"/>
		<rdfs:label>twelve months</rdfs:label>
		<skos:definition>a duration of exactly twelve (12) months, regardless of the length in days of a given calendar month, but typically 30 days</skos:definition>
		<fibo-fnd-dt-fd:hasDurationValue>P12M</fibo-fnd-dt-fd:hasDurationValue>
	</fibo-fnd-dt-fd:ExplicitDuration>
	
	<fibo-fnd-dt-fd:ExplicitDuration
		rdf:about="&fibo-ind-ir-ir;TwentyFourMonths">
		<rdf:type
			rdf:resource="&owl;NamedIndividual"/>
		<rdfs:label>twenty-four months</rdfs:label>
		<skos:definition>a duration of exactly twenty-four (24) months, regardless of the length in days of a given calendar month, but typically 30 days</skos:definition>
		<fibo-fnd-dt-fd:hasDurationValue>P24M</fibo-fnd-dt-fd:hasDurationValue>
	</fibo-fnd-dt-fd:ExplicitDuration>
	
	<fibo-fnd-dt-fd:ExplicitDuration
		rdf:about="&fibo-ind-ir-ir;TwentyYears">
		<rdf:type
			rdf:resource="&owl;NamedIndividual"/>
		<rdfs:label>twenty years</rdfs:label>
		<skos:definition>a duration of exactly twenty (20) years</skos:definition>
		<fibo-fnd-dt-fd:hasDurationValue>P20Y</fibo-fnd-dt-fd:hasDurationValue>
	</fibo-fnd-dt-fd:ExplicitDuration>
	
	<fibo-fnd-dt-fd:ExplicitDuration
		rdf:about="&fibo-ind-ir-ir;TwoMonths">
		<rdf:type
			rdf:resource="&owl;NamedIndividual"/>
		<rdfs:label>two months</rdfs:label>
		<skos:definition>a duration of exactly two (2) months, regardless of the length in days of a given calendar month, but typically 30 days</skos:definition>
		<fibo-fnd-dt-fd:hasDurationValue>P2M</fibo-fnd-dt-fd:hasDurationValue>
	</fibo-fnd-dt-fd:ExplicitDuration>
	
	<fibo-fnd-dt-fd:ExplicitDuration
		rdf:about="&fibo-ind-ir-ir;TwoYears">
		<rdf:type
			rdf:resource="&owl;NamedIndividual"/>
		<rdfs:label>two years</rdfs:label>
		<skos:definition>a duration of exactly two (2) years</skos:definition>
		<fibo-fnd-dt-fd:hasDurationValue>P2Y</fibo-fnd-dt-fd:hasDurationValue>
	</fibo-fnd-dt-fd:ExplicitDuration>
	
	<owl:ObjectProperty
		rdf:about="&fibo-ind-ir-ir;hasRateResetTimeOfDay">
		<rdfs:subPropertyOf
			rdf:resource="&fibo-fnd-dt-fd;hasDateTime"/>
		<rdfs:label>has rate reset time of day</rdfs:label>
		<rdfs:range
			rdf:resource="&fibo-fnd-dt-fd;DateTime"/>
		<skos:definition>indicates the time of day when a rate is reset</skos:definition>
	</owl:ObjectProperty>
	
	<owl:ObjectProperty
		rdf:about="&fibo-ind-ir-ir;hasReferenceCurrency">
		<rdfs:subPropertyOf
			rdf:resource="&fibo-fnd-rel-rel;has"/>
		<rdfs:label>has reference currency</rdfs:label>
		<rdfs:domain
			rdf:resource="&fibo-ind-ir-ir;ReferenceInterestRate"/>
		<rdfs:range
			rdf:resource="&fibo-fnd-acc-cur;Currency"/>
		<skos:definition>relates a reference rate to the currency it is based on</skos:definition>
	</owl:ObjectProperty>
	
	<owl:ObjectProperty
		rdf:about="&fibo-ind-ir-ir;hasTenor">
		<rdfs:subPropertyOf
			rdf:resource="&fibo-fnd-dt-fd;hasDuration"/>
		<rdfs:label>has tenor</rdfs:label>
		<rdfs:range
			rdf:resource="&fibo-fnd-dt-fd;Duration"/>
		<skos:definition>indicates the length of time for which a given rate, such as an interbank rate, exchange rate, other market rate is quoted, or a debt instrument has remaining prior to maturity or expiration</skos:definition>
		<skos:example>The length of time until a loan is due. For example, a loan is taken out with a two year tenor. After one year passes, the tenor of the loan is one year.</skos:example>
		<fibo-fnd-utl-av:adaptedFrom
			rdf:datatype="&xsd;anyURI">http://www.investopedia.com/terms/t/tenor.asp</fibo-fnd-utl-av:adaptedFrom>
		<fibo-fnd-utl-av:explanatoryNote>The tenor of most financial instruments declines over time, while the maturity remains constant. Risk associated with a given asset tends to decline with the reduction of the time remaining to maturity. The tenor of an interest rate swap can also refer to the frequency with which coupon payments are exchanged.</fibo-fnd-utl-av:explanatoryNote>
	</owl:ObjectProperty>
	
	<owl:DatatypeProperty
		rdf:about="&fibo-ind-ir-ir;hasTenorInDays">
		<rdfs:label>has tenor in days</rdfs:label>
		<rdfs:domain
			rdf:resource="&fibo-ind-ir-ir;InterbankRate"/>
		<rdfs:range
			rdf:resource="&xsd;integer"/>
		<owl:deprecated
			rdf:datatype="&xsd;boolean">true</owl:deprecated>
		<skos:definition>a predicate indicating the length of time for which the interbank rate is quoted expressed as a number of days</skos:definition>
		<skos:editorialNote>This is given as a whole number representing the number of days, because the concept of a duration is not yet modeled semantically, otherwise this term would refer to duration as its range instead. The name of this property reflects this compromise and would be changed to &quot;Tenor&quot; once a suitable range exists for this property.</skos:editorialNote>
	</owl:DatatypeProperty>
	
	<owl:DatatypeProperty
		rdf:about="&fibo-ind-ir-ir;hasTenorInMonths">
		<rdfs:label>has tenor in months</rdfs:label>
		<rdfs:domain
			rdf:resource="&fibo-ind-ir-ir;InterbankRate"/>
		<rdfs:range
			rdf:resource="&xsd;integer"/>
		<owl:deprecated
			rdf:datatype="&xsd;boolean">true</owl:deprecated>
		<skos:definition>a predicate indicating the length of time for which the interbank rate is quoted, e.g., 3 months, 6 months expressed as a number of months</skos:definition>
	</owl:DatatypeProperty>

</rdf:RDF>