<?xml version="1.0" encoding="UTF-8"?>
  
<!DOCTYPE rdf:RDF [
    <!ENTITY fibo-md-tmp-crr "http://spec.edmcouncil.org/fibo/red/md/temporal-core/credit-ratings/">
    <!ENTITY fibo-fnd-info-sch "http://spec.edmcouncil.org/fibo/red/fnd/information/schemes/">
    <!ENTITY fibo-fnd-info-tem "http://spec.edmcouncil.org/fibo/red/fnd/information/temporal-info/">
    <!ENTITY fibo-fnd-pub-pub "http://spec.edmcouncil.org/fibo/red/fnd/publications/publications/">
    <!ENTITY fibo-sec-sec-iss "http://spec.edmcouncil.org/fibo/red/sec/securities/securities-issuance-terms/">
    <!ENTITY fibo-be-le-fbo "http://spec.edmcouncil.org/fibo/red/be/legal-entities/formal-business-organizations/">
    <!ENTITY fibo-sec-sec-sec "http://spec.edmcouncil.org/fibo/red/sec/securities/securities/">
    <!ENTITY fibo-uo-lat "http://spec.edmcouncil.org/fibo/red/uo/lattice/">
]>

<rdf:RDF xmlns:xsd="http://www.w3.org/2001/XMLSchema#"
         xmlns:sm="http://www.omg.org/techprocess/ab/SpecificationMetadata/"
         xmlns:xs="http://www.w3.org/2001/XMLSchema"
         xmlns:fibo-fnd-utl-av="http://www.omg.org/spec/EDMC-FIBO/FND/Utilities/AnnotationVocabulary/"
         xmlns:rdf="http://www.w3.org/1999/02/22-rdf-syntax-ns#"
         xmlns:rdfs="http://www.w3.org/2000/01/rdf-schema#"
         xmlns:owl="http://www.w3.org/2002/07/owl#"
         xmlns:skos="http://www.w3.org/2004/02/skos/core#"
         xmlns:dc="http://purl.org/dc/terms/"
         xml:base="http://spec.edmcouncil.org/fibo/red/md/temporal-core/credit-ratings/">

   <owl:Ontology rdf:about="http://spec.edmcouncil.org/fibo/red/md/temporal-core/credit-ratings/">
      <owl:imports rdf:resource="http://spec.edmcouncil.org/fibo/red/fnd/information/schemes/"/>
      <owl:imports rdf:resource="http://spec.edmcouncil.org/fibo/red/fnd/information/temporal-info/"/>
      <owl:imports rdf:resource="http://spec.edmcouncil.org/fibo/red/fnd/publications/publications/"/>
      <owl:imports rdf:resource="http://spec.edmcouncil.org/fibo/red/sec/securities/securities-issuance-terms/"/>
      <owl:imports rdf:resource="http://spec.edmcouncil.org/fibo/red/be/legal-entities/formal-business-organizations/"/>
      <owl:imports rdf:resource="http://spec.edmcouncil.org/fibo/red/sec/securities/securities/"/>
      <owl:imports rdf:resource="http://spec.edmcouncil.org/fibo/red/uo/lattice/"/>
   </owl:Ontology>


  <!--
    ///////////////////////////////////////////////////////////////////////////////////////
    //
    // Datatypes
    //
    ///////////////////////////////////////////////////////////////////////////////////////
    -->


<rdfs:Datatype rdf:about="&fibo-md-tmp-crr;CreditWatchDirectionSelection">
      <owl:equivalentClass>
         <rdfs:Datatype>
            <owl:oneOf>
               <rdf:Description>
                  <rdf:first rdf:datatype="http://www.w3.org/2001/XMLSchema#string">Upgrade</rdf:first>
                  <rdf:rest>
                     <rdf:Description>
                        <rdf:first rdf:datatype="http://www.w3.org/2001/XMLSchema#string">Downgrade</rdf:first>
                        <rdf:rest rdf:resource="http://www.w3.org/1999/02/22-rdf-syntax-ns#nil"/>
                     </rdf:Description>
                  </rdf:rest>
               </rdf:Description>
            </owl:oneOf>
         </rdfs:Datatype>
      </owl:equivalentClass>
   </rdfs:Datatype>

   <rdfs:Datatype rdf:about="&fibo-md-tmp-crr;CreditWatchOutlookSelection">
      <owl:equivalentClass>
         <rdfs:Datatype>
            <owl:oneOf>
               <rdf:Description>
                  <rdf:first rdf:datatype="http://www.w3.org/2001/XMLSchema#string">Stable</rdf:first>
                  <rdf:rest>
                     <rdf:Description>
                        <rdf:first rdf:datatype="http://www.w3.org/2001/XMLSchema#string">On Watch</rdf:first>
                        <rdf:rest rdf:resource="http://www.w3.org/1999/02/22-rdf-syntax-ns#nil"/>
                     </rdf:Description>
                  </rdf:rest>
               </rdf:Description>
            </owl:oneOf>
         </rdfs:Datatype>
      </owl:equivalentClass>
   </rdfs:Datatype>


  <!--
    ///////////////////////////////////////////////////////////////////////////////////////
    //
    // Object Properties
    //
    ///////////////////////////////////////////////////////////////////////////////////////
    -->


<owl:ObjectProperty rdf:about="&fibo-md-tmp-crr;definedIn">
      <rdfs:label>defined in</rdfs:label>
      <rdfs:subPropertyOf rdf:resource="&fibo-fnd-info-sch;definedIn"/>
      <rdfs:domain rdf:resource="&fibo-md-tmp-crr;InvestmentCreditRating"/>
      <rdfs:range rdf:resource="&fibo-md-tmp-crr;CreditRatingScheme"/>
   </owl:ObjectProperty>

   <owl:ObjectProperty rdf:about="&fibo-md-tmp-crr;rates">
      <rdfs:label>rates</rdfs:label>
      <rdfs:subPropertyOf rdf:resource="&fibo-md-tmp-crr;rates.1"/>
      <rdfs:domain rdf:resource="&fibo-md-tmp-crr;IssueCreditRating"/>
      <rdfs:range rdf:resource="&fibo-sec-sec-iss;OfferIssue"/>
   </owl:ObjectProperty>

   <owl:ObjectProperty rdf:about="&fibo-md-tmp-crr;rated">
      <rdfs:label>rated</rdfs:label>
      <rdfs:domain rdf:resource="&fibo-sec-sec-sec;Security"/>
      <rdfs:range rdf:resource="&fibo-md-tmp-crr;InstrumentCreditRating"/>
   </owl:ObjectProperty>

   <owl:ObjectProperty rdf:about="&fibo-md-tmp-crr;issuedBy">
      <rdfs:label>issued by</rdfs:label>
      <rdfs:subPropertyOf rdf:resource="&fibo-fnd-pub-pub;publishedBy"/>
      <rdfs:domain rdf:resource="&fibo-md-tmp-crr;InvestmentCreditRating"/>
      <rdfs:range rdf:resource="&fibo-md-tmp-crr;CreditRatingIssuer"/>
   </owl:ObjectProperty>

   <owl:ObjectProperty rdf:about="&fibo-md-tmp-crr;rates.1">
      <rdfs:label>rates</rdfs:label>
      <skos:definition>The Credit rating rates something, for example a legal entity, an instrument or some such. The thing that can be rated is any type of Continuant Thing.</skos:definition>
      <rdfs:subPropertyOf rdf:resource="&fibo-fnd-pub-pub;isAbout"/>
      <rdfs:domain rdf:resource="&fibo-md-tmp-crr;InvestmentCreditRating"/>
      <rdfs:range rdf:resource="&fibo-uo-lat;ContinuantThing"/>
   </owl:ObjectProperty>

   <owl:ObjectProperty rdf:about="&fibo-md-tmp-crr;rates.2">
      <rdfs:label>rates</rdfs:label>
      <rdfs:subPropertyOf rdf:resource="&fibo-md-tmp-crr;rates.1"/>
      <rdfs:domain rdf:resource="&fibo-md-tmp-crr;InstrumentCreditRating"/>
      <rdfs:range rdf:resource="&fibo-sec-sec-sec;Security"/>
      <owl:inverseOf rdf:resource="&fibo-md-tmp-crr;rated"/>
   </owl:ObjectProperty>

   <owl:ObjectProperty rdf:about="&fibo-md-tmp-crr;rates.3">
      <rdfs:label>rates</rdfs:label>
      <rdfs:subPropertyOf rdf:resource="&fibo-md-tmp-crr;rates.1"/>
      <rdfs:domain rdf:resource="&fibo-md-tmp-crr;OrganizationCreditRating"/>
      <rdfs:range rdf:resource="&fibo-be-le-fbo;FormallyConstitutedOrganization"/>
   </owl:ObjectProperty>

   <owl:ObjectProperty rdf:about="&fibo-md-tmp-crr;hasIdentity">
      <rdfs:label>has identity</rdfs:label>
      <rdfs:subPropertyOf rdf:resource="&fibo-fnd-pub-pub;publisherIdentity"/>
      <rdfs:domain rdf:resource="&fibo-md-tmp-crr;CreditRatingIssuer"/>
      <rdfs:range rdf:resource="&fibo-md-tmp-crr;CreditRatingAgency"/>
   </owl:ObjectProperty>


  <!--
    ///////////////////////////////////////////////////////////////////////////////////////
    //
    // Data Properties
    //
    ///////////////////////////////////////////////////////////////////////////////////////
    -->


<owl:DatatypeProperty rdf:about="&fibo-md-tmp-crr;watchDirection">
      <rdfs:label>watch direction</rdfs:label>
      <skos:definition>The direction in which the credit rating is expected to move, for something which has a credit rating on watch.</skos:definition>
      <rdfs:range rdf:resource="&fibo-md-tmp-crr;CreditWatchDirectionSelection"/>
   </owl:DatatypeProperty>

   <owl:DatatypeProperty rdf:about="&fibo-md-tmp-crr;watchOutlook">
      <rdfs:label>watch outlook</rdfs:label>
      <skos:definition>The expected outlook for the rated entity.</skos:definition>
      <rdfs:range rdf:resource="&fibo-md-tmp-crr;CreditWatchOutlookSelection"/>
   </owl:DatatypeProperty>


  <!--
    ///////////////////////////////////////////////////////////////////////////////////////
    //
    // Annotation Properties
    //
    ///////////////////////////////////////////////////////////////////////////////////////
    -->



  <!--
    ///////////////////////////////////////////////////////////////////////////////////////
    //
    // Classes
    //
    ///////////////////////////////////////////////////////////////////////////////////////
    -->


<owl:Class rdf:about="&fibo-md-tmp-crr;CreditRating">
      <rdfs:label>credit rating</rdfs:label>
      <skos:definition>Some rating which formally describes the credit worthiness of something or someone.</skos:definition>
      <rdfs:subClassOf rdf:resource="&fibo-fnd-info-tem;Rating"/>
   </owl:Class>

   <owl:Class rdf:about="&fibo-md-tmp-crr;CreditRatingScheme">
      <rdfs:label>credit rating scheme</rdfs:label>
      <skos:definition>The scheme which defines what rating codes exist and what judgements each one represents, as defined by the Rating agency.</skos:definition>
      <rdfs:subClassOf rdf:resource="&fibo-fnd-info-sch;Scheme"/>
   </owl:Class>

   <owl:Class rdf:about="&fibo-md-tmp-crr;IndividualCreditRating">
      <rdfs:label>individual credit rating</rdfs:label>
      <rdfs:subClassOf rdf:resource="&fibo-md-tmp-crr;CreditRating"/>
   </owl:Class>

   <owl:Class rdf:about="&fibo-md-tmp-crr;IssueCreditRating">
      <rdfs:label>issue credit rating</rdfs:label>
      <skos:definition>The creditworthiness of the overall issue as determined by a Ratings Agency.</skos:definition>
      <rdfs:subClassOf rdf:resource="&fibo-md-tmp-crr;InvestmentCreditRating"/>
   </owl:Class>

   <owl:Class rdf:about="&fibo-md-tmp-crr;ShortTermCreditRating">
      <rdfs:label>short term credit rating</rdfs:label>
      <skos:definition>A short term rating is a probability factor of an individual going into default within a year. This is in contrast to long-term rating which is evaluated over a long timeframe.</skos:definition>
   </owl:Class>

   <owl:Class rdf:about="&fibo-md-tmp-crr;InvestmentCreditRating">
      <rdfs:label>investment credit rating</rdfs:label>
      <skos:definition>The creditworthiness of an investment as determined by a Ratings Agency. Further notes: Anything can be bought and sold can have a rating. Credit rating can be assigned to an instrument, an organization, even a person. The rating is assigned to any kind of instrument that the organization etc. issues. Use Wikipedia credit rating definition Long term, short term and generic ratings The rating differentiates between short and long term (not sure about generic). In all systems these are differentiated. This relates to how long the holder might hold the thing. Or does it? The agencies offer two different servies and you pay 2 different fees for short and long. ACTION: to find The codes themselves are different. So it's not AAA etc. for short term it's something else. so the thing we've been thinking about is actually long term ratings.</skos:definition>
      <rdfs:subClassOf rdf:resource="&fibo-fnd-pub-pub;PublishedInformation"/>
   </owl:Class>

   <owl:Class rdf:about="&fibo-md-tmp-crr;InstrumentCreditRating">
      <rdfs:label>instrument credit rating</rdfs:label>
      <skos:definition>An Instrument Credit Rating, that is the creditworthiness of the investment as determined by a Ratings Agency.</skos:definition>
   </owl:Class>

   <owl:Class rdf:about="&fibo-md-tmp-crr;OrganizationCreditRating">
      <rdfs:label>organization credit rating</rdfs:label>
      <skos:definition>The credit rating of the organization. That is the creditworthiness of the organization as determined by a ratings agency. If the organization is the issuer of a security then this becomes the issuer rating for that security.</skos:definition>
      <rdfs:subClassOf rdf:resource="&fibo-md-tmp-crr;IndividualCreditRating"/>
   </owl:Class>

   <owl:Class rdf:about="&fibo-md-tmp-crr;CreditRatingAgency">
      <rdfs:label>credit rating agency</rdfs:label>
      <skos:definition>An entity which publishes Credit Ratings.</skos:definition>
      <rdfs:subClassOf rdf:resource="&fibo-fnd-pub-pub;PublishingHouse"/>
   </owl:Class>

   <owl:Class rdf:about="&fibo-md-tmp-crr;CreditRatingIssuer">
      <rdfs:label>credit rating issuer</rdfs:label>
      <skos:definition>An entity which publishes credit ratings for business entities and / or securities Further notes: This entity also defines the meanings (judgements) represented by each Ratings code as documented in the Credit Rating Scheme. .</skos:definition>
      <rdfs:subClassOf rdf:resource="&fibo-fnd-pub-pub;Publisher"/>
   </owl:Class>


  <!--
    ///////////////////////////////////////////////////////////////////////////////////////
    //
    // Individuals
    //
    ///////////////////////////////////////////////////////////////////////////////////////
    -->


</rdf:RDF>