<?xml version="1.0" encoding="UTF-8"?>
  
<!DOCTYPE rdf:RDF [
    <!ENTITY fibo-loan-typ-cr "http://spec.edmcouncil.org/fibo/red/loan/loan-types/credit-products/">
    <!ENTITY fibo-fnd-acc-crf "http://spec.edmcouncil.org/fibo/red/fnd/accounting/credit-facilities/">
    <!ENTITY fibo-fnd-acc-dbt "http://spec.edmcouncil.org/fibo/red/fnd/accounting/debt-terms/">
    <!ENTITY fibo-loan-loan-col "http://spec.edmcouncil.org/fibo/red/loan/loans/loans-collateral/">
    <!ENTITY fibo-fnd-acc-cur "http://spec.edmcouncil.org/fibo/red/fnd/accounting/currency-amount/">
]>

<rdf:RDF xmlns:xsd="http://www.w3.org/2001/XMLSchema#"
         xmlns:sm="http://www.omg.org/techprocess/ab/SpecificationMetadata/"
         xmlns:xs="http://www.w3.org/2001/XMLSchema"
         xmlns:fibo-fnd-utl-av="http://www.omg.org/spec/EDMC-FIBO/FND/Utilities/AnnotationVocabulary/"
         xmlns:rdf="http://www.w3.org/1999/02/22-rdf-syntax-ns#"
         xmlns:rdfs="http://www.w3.org/2000/01/rdf-schema#"
         xmlns:owl="http://www.w3.org/2002/07/owl#"
         xmlns:skos="http://www.w3.org/2004/02/skos/core#"
         xmlns:dc="http://purl.org/dc/terms/"
         xml:base="http://spec.edmcouncil.org/fibo/red/loan/loan-types/credit-products/">

   <owl:Ontology rdf:about="http://spec.edmcouncil.org/fibo/red/loan/loan-types/credit-products/">
      <owl:imports rdf:resource="http://spec.edmcouncil.org/fibo/red/fnd/accounting/credit-facilities/"/>
      <owl:imports rdf:resource="http://spec.edmcouncil.org/fibo/red/fnd/accounting/debt-terms/"/>
      <owl:imports rdf:resource="http://spec.edmcouncil.org/fibo/red/loan/loans/loans-collateral/"/>
      <owl:imports rdf:resource="http://spec.edmcouncil.org/fibo/red/fnd/accounting/currency-amount/"/>
   </owl:Ontology>


  <!--
    ///////////////////////////////////////////////////////////////////////////////////////
    //
    // Datatypes
    //
    ///////////////////////////////////////////////////////////////////////////////////////
    -->



  <!--
    ///////////////////////////////////////////////////////////////////////////////////////
    //
    // Object Properties
    //
    ///////////////////////////////////////////////////////////////////////////////////////
    -->


<owl:ObjectProperty rdf:about="&fibo-loan-typ-cr;setsOutTermsFor">
      <rdfs:label>sets out terms for</rdfs:label>
      <rdfs:subPropertyOf rdf:resource="&fibo-fnd-acc-crf;setsOutTermsFor"/>
      <rdfs:domain rdf:resource="&fibo-loan-typ-cr;HomeEquityLineOfCreditContract"/>
      <rdfs:range rdf:resource="&fibo-loan-typ-cr;HomeEquityLineOfCredit"/>
   </owl:ObjectProperty>

   <owl:ObjectProperty rdf:about="&fibo-loan-typ-cr;collateralizedBy">
      <rdfs:label>collateralized by</rdfs:label>
      <rdfs:subPropertyOf rdf:resource="&fibo-loan-typ-cr;collateralizedBy.1"/>
      <rdfs:domain rdf:resource="&fibo-loan-typ-cr;HomeEquityLineOfCredit"/>
      <rdfs:range rdf:resource="&fibo-loan-loan-col;LoanPropertyCollateral"/>
   </owl:ObjectProperty>

   <owl:ObjectProperty rdf:about="&fibo-loan-typ-cr;maximumAllowedBalance">
      <rdfs:label>maximum allowed balance</rdfs:label>
      <skos:definition>The maximum loan amount that is allowed to be outstanding as defined in this loan contract.</skos:definition>
      <rdfs:domain rdf:resource="&fibo-loan-typ-cr;RevolvingCreditContract"/>
      <rdfs:range rdf:resource="&fibo-fnd-acc-cur;MoneyAmount"/>
   </owl:ObjectProperty>

   <owl:ObjectProperty rdf:about="&fibo-loan-typ-cr;maximumAnticipatedBalance">
      <rdfs:label>maximum anticipated balance</rdfs:label>
      <skos:definition>The maximum loan amount that could potentially be outstanding.</skos:definition>
      <rdfs:domain rdf:resource="&fibo-loan-typ-cr;RevolvingLineOfCredit"/>
      <rdfs:range rdf:resource="&fibo-fnd-acc-cur;MoneyAmount"/>
   </owl:ObjectProperty>

   <owl:ObjectProperty rdf:about="&fibo-loan-typ-cr;setsOutTermsFor.1">
      <rdfs:label>sets out terms for</rdfs:label>
      <rdfs:subPropertyOf rdf:resource="&fibo-fnd-acc-crf;setsOutTermsFor"/>
      <rdfs:domain rdf:resource="&fibo-loan-typ-cr;RevolvingCreditContract"/>
      <rdfs:range rdf:resource="&fibo-loan-typ-cr;RevolvingLineOfCredit"/>
   </owl:ObjectProperty>

   <owl:ObjectProperty rdf:about="&fibo-loan-typ-cr;collateralizedBy.1">
      <rdfs:label>collateralized by</rdfs:label>
      <rdfs:subPropertyOf rdf:resource="&fibo-fnd-acc-dbt;collateralizedBy"/>
      <rdfs:domain rdf:resource="&fibo-loan-typ-cr;RevolvingLineOfCredit"/>
      <rdfs:range rdf:resource="&fibo-loan-loan-col;LoanCollateral"/>
   </owl:ObjectProperty>


  <!--
    ///////////////////////////////////////////////////////////////////////////////////////
    //
    // Data Properties
    //
    ///////////////////////////////////////////////////////////////////////////////////////
    -->



  <!--
    ///////////////////////////////////////////////////////////////////////////////////////
    //
    // Annotation Properties
    //
    ///////////////////////////////////////////////////////////////////////////////////////
    -->



  <!--
    ///////////////////////////////////////////////////////////////////////////////////////
    //
    // Classes
    //
    ///////////////////////////////////////////////////////////////////////////////////////
    -->


<owl:Class rdf:about="&fibo-loan-typ-cr;CreditCard">
      <rdfs:label>credit card</rdfs:label>
      <rdfs:subClassOf rdf:resource="&fibo-fnd-acc-crf;CommittedCreditFacilityTranche"/>
   </owl:Class>

   <owl:Class rdf:about="&fibo-loan-typ-cr;HomeEquityLineOfCredit">
      <rdfs:label>home equity line of credit</rdfs:label>
      <skos:definition>A credit line on a house or other property, that can be drawn down and/or paid back by the borrower.</skos:definition>
      <rdfs:subClassOf rdf:resource="&fibo-loan-typ-cr;RevolvingLineOfCredit"/>
   </owl:Class>

   <owl:Class rdf:about="&fibo-loan-typ-cr;HomeEquityLineOfCreditContract">
      <rdfs:label>home equity line of credit contract</rdfs:label>
      <skos:definition>A credit line on a house or other property, that can be drawn down and/or paid back by the borrower.</skos:definition>
      <rdfs:subClassOf rdf:resource="&fibo-loan-typ-cr;RevolvingCreditContract"/>
   </owl:Class>

   <owl:Class rdf:about="&fibo-loan-typ-cr;RevolvingCreditContract">
      <rdfs:label>revolving credit contract</rdfs:label>
      <skos:definition>Contract which embodies and defines the terms and conditions for a credit line based on some collaterial, which can be drawn down and/or paid back by the borrower.</skos:definition>
      <rdfs:subClassOf rdf:resource="&fibo-fnd-acc-crf;CreditFacilityAgreement"/>
   </owl:Class>

   <owl:Class rdf:about="&fibo-loan-typ-cr;RevolvingLineOfCredit">
      <rdfs:label>revolving line of credit</rdfs:label>
      <skos:definition>A credit line based on some collateral, that can be drawn down and/or paid back by the borrower.</skos:definition>
   </owl:Class>


  <!--
    ///////////////////////////////////////////////////////////////////////////////////////
    //
    // Individuals
    //
    ///////////////////////////////////////////////////////////////////////////////////////
    -->


</rdf:RDF>