<?xml version="1.0" encoding="UTF-8"?>
  
<!DOCTYPE rdf:RDF [
    <!ENTITY fibo-sec-eq-shr "http://spec.edmcouncil.org/fibo/red/sec/equities/shareholder-rights/">
    <!ENTITY fibo-sec-eq-eqi "http://spec.edmcouncil.org/fibo/red/sec/equities/equity-instruments/">
    <!ENTITY fibo-fnd-agrx-cst "http://spec.edmcouncil.org/fibo/red/fnd/agreements-ext/contractual-constructs/">
    <!ENTITY fibo-sec-eq-sh "http://spec.edmcouncil.org/fibo/red/sec/equities/share-terms/">
]>

<rdf:RDF xmlns:xsd="http://www.w3.org/2001/XMLSchema#"
         xmlns:sm="http://www.omg.org/techprocess/ab/SpecificationMetadata/"
         xmlns:xs="http://www.w3.org/2001/XMLSchema"
         xmlns:fibo-fnd-utl-av="http://www.omg.org/spec/EDMC-FIBO/FND/Utilities/AnnotationVocabulary/"
         xmlns:rdf="http://www.w3.org/1999/02/22-rdf-syntax-ns#"
         xmlns:rdfs="http://www.w3.org/2000/01/rdf-schema#"
         xmlns:owl="http://www.w3.org/2002/07/owl#"
         xmlns:skos="http://www.w3.org/2004/02/skos/core#"
         xmlns:dc="http://purl.org/dc/terms/"
         xml:base="http://spec.edmcouncil.org/fibo/red/sec/equities/shareholder-rights/">

   <owl:Ontology rdf:about="http://spec.edmcouncil.org/fibo/red/sec/equities/shareholder-rights/">
      <owl:imports rdf:resource="http://spec.edmcouncil.org/fibo/red/sec/equities/equity-instruments/"/>
      <owl:imports rdf:resource="http://spec.edmcouncil.org/fibo/red/fnd/agreements-ext/contractual-constructs/"/>
      <owl:imports rdf:resource="http://spec.edmcouncil.org/fibo/red/sec/equities/share-terms/"/>
   </owl:Ontology>


  <!--
    ///////////////////////////////////////////////////////////////////////////////////////
    //
    // Datatypes
    //
    ///////////////////////////////////////////////////////////////////////////////////////
    -->



  <!--
    ///////////////////////////////////////////////////////////////////////////////////////
    //
    // Object Properties
    //
    ///////////////////////////////////////////////////////////////////////////////////////
    -->


<owl:ObjectProperty rdf:about="&fibo-sec-eq-shr;setsOut">
      <rdfs:label>sets out</rdfs:label>
      <rdfs:subPropertyOf rdf:resource="&fibo-fnd-agrx-cst;setsOutRight"/>
      <rdfs:domain rdf:resource="&fibo-sec-eq-shr;EquityVotingRightsTermsSet"/>
      <rdfs:range rdf:resource="&fibo-sec-eq-eqi;VotingRight"/>
   </owl:ObjectProperty>

   <owl:ObjectProperty rdf:about="&fibo-sec-eq-shr;mayConfer">
      <rdfs:label>may confer</rdfs:label>
      <skos:definition>The right of the holder of the Preference Shares to vote on matters affecting the business of the issuing company. A preference share may confer some voting rights whereby the holder may vote in extraordinary general meetings. These are not the same as the ordinary voting rights conferred by ordinary shares.</skos:definition>
      <rdfs:subPropertyOf rdf:resource="&fibo-sec-eq-eqi;shareConfers"/>
      <rdfs:domain rdf:resource="&fibo-sec-eq-sh;PreferenceShare"/>
      <rdfs:range rdf:resource="&fibo-sec-eq-shr;ExtraordinaryVotingRight"/>
   </owl:ObjectProperty>


  <!--
    ///////////////////////////////////////////////////////////////////////////////////////
    //
    // Data Properties
    //
    ///////////////////////////////////////////////////////////////////////////////////////
    -->


<owl:DatatypeProperty rdf:about="&fibo-sec-eq-shr;typeOfVotingRights">
      <rdfs:label>type of voting rights</rdfs:label>
      <skos:definition>The specification of voting rights for the security, in this case extraordinary voting rights.</skos:definition>
      <rdfs:range rdf:resource="&fibo-sec-eq-eqi;VotingRightsTypeSelection"/>
   </owl:DatatypeProperty>

   <owl:DatatypeProperty rdf:about="&fibo-sec-eq-shr;typeOfVotingRights.1">
      <rdfs:label>type of voting rights</rdfs:label>
      <skos:definition>The specification of voting rights for the security. These are defined as Ordinary voting rights, which give the holder the right to vote at meetings of the company along with other shareholders, on matters of policy and direction and the election of office bearers.</skos:definition>
      <rdfs:range rdf:resource="&fibo-sec-eq-eqi;VotingRightsTypeSelection"/>
   </owl:DatatypeProperty>


  <!--
    ///////////////////////////////////////////////////////////////////////////////////////
    //
    // Annotation Properties
    //
    ///////////////////////////////////////////////////////////////////////////////////////
    -->



  <!--
    ///////////////////////////////////////////////////////////////////////////////////////
    //
    // Classes
    //
    ///////////////////////////////////////////////////////////////////////////////////////
    -->


<owl:Class rdf:about="&fibo-sec-eq-shr;EquityVotingRightsTermsSet">
      <rdfs:label>equity voting rights terms set</rdfs:label>
      <skos:definition>Terms setting out the voting rights of the Holder.</skos:definition>
      <rdfs:subClassOf rdf:resource="&fibo-sec-eq-sh;CompanyEquityTermsSet"/>
   </owl:Class>

   <owl:Class rdf:about="&fibo-sec-eq-shr;ExtraordinaryVotingRight">
      <rdfs:label>extraordinary voting right</rdfs:label>
      <skos:definition>The right to vote at extraordinary meetings, as opposed to being able to vote at annual general meetings.</skos:definition>
      <rdfs:subClassOf rdf:resource="&fibo-sec-eq-eqi;VotingRight"/>
   </owl:Class>

   <owl:Class rdf:about="&fibo-sec-eq-shr;OrdinaryVotingRight">
      <rdfs:label>ordinary voting right</rdfs:label>
      <skos:definition>The voting rights conferred on holders of Ordinary Shares in the company. The precise details of these rights such as what shareholders may vote on and how their voting right is exercised, are defined in the Company Constitution or Articles of Incorporation / Articles of Association.</skos:definition>
   </owl:Class>


  <!--
    ///////////////////////////////////////////////////////////////////////////////////////
    //
    // Individuals
    //
    ///////////////////////////////////////////////////////////////////////////////////////
    -->


</rdf:RDF>