<?xml version="1.0" encoding="UTF-8"?>
  
<!DOCTYPE rdf:RDF [
    <!ENTITY fibo-sec-eq-she "http://spec.edmcouncil.org/fibo/red/sec/equities/shareholder-equity/">
    <!ENTITY fibo-sec-eq-eqi "http://spec.edmcouncil.org/fibo/red/sec/equities/equity-instruments/">
    <!ENTITY fibo-sec-eq-sh "http://spec.edmcouncil.org/fibo/red/sec/equities/share-terms/">
    <!ENTITY fibo-fnd-law-lcap "http://spec.edmcouncil.org/fibo/red/fnd/law/legal-capacities/">
    <!ENTITY fibo-fnd-agrx-cst "http://spec.edmcouncil.org/fibo/red/fnd/agreements-ext/contractual-constructs/">
    <!ENTITY fibo-be-oac-exec "http://spec.edmcouncil.org/fibo/red/be/ownership-and-control/executives/">
]>

<rdf:RDF xmlns:xsd="http://www.w3.org/2001/XMLSchema#"
         xmlns:sm="http://www.omg.org/techprocess/ab/SpecificationMetadata/"
         xmlns:xs="http://www.w3.org/2001/XMLSchema"
         xmlns:fibo-fnd-utl-av="http://www.omg.org/spec/EDMC-FIBO/FND/Utilities/AnnotationVocabulary/"
         xmlns:rdf="http://www.w3.org/1999/02/22-rdf-syntax-ns#"
         xmlns:rdfs="http://www.w3.org/2000/01/rdf-schema#"
         xmlns:owl="http://www.w3.org/2002/07/owl#"
         xmlns:skos="http://www.w3.org/2004/02/skos/core#"
         xmlns:dc="http://purl.org/dc/terms/"
         xml:base="http://spec.edmcouncil.org/fibo/red/sec/equities/shareholder-equity/">

   <owl:Ontology rdf:about="http://spec.edmcouncil.org/fibo/red/sec/equities/shareholder-equity/">
      <owl:imports rdf:resource="http://spec.edmcouncil.org/fibo/red/sec/equities/equity-instruments/"/>
      <owl:imports rdf:resource="http://spec.edmcouncil.org/fibo/red/sec/equities/share-terms/"/>
      <owl:imports rdf:resource="http://spec.edmcouncil.org/fibo/red/fnd/law/legal-capacities/"/>
      <owl:imports rdf:resource="http://spec.edmcouncil.org/fibo/red/fnd/agreements-ext/contractual-constructs/"/>
      <owl:imports rdf:resource="http://spec.edmcouncil.org/fibo/red/be/ownership-and-control/executives/"/>
   </owl:Ontology>


  <!--
    ///////////////////////////////////////////////////////////////////////////////////////
    //
    // Datatypes
    //
    ///////////////////////////////////////////////////////////////////////////////////////
    -->



  <!--
    ///////////////////////////////////////////////////////////////////////////////////////
    //
    // Object Properties
    //
    ///////////////////////////////////////////////////////////////////////////////////////
    -->


<owl:ObjectProperty rdf:about="&fibo-sec-eq-she;confers">
      <rdfs:label>confers</rdfs:label>
      <rdfs:subPropertyOf rdf:resource="&fibo-fnd-agrx-cst;setsOutRight"/>
      <rdfs:domain rdf:resource="&fibo-sec-eq-she;EquityPriorityTermsSet"/>
      <rdfs:range rdf:resource="&fibo-sec-eq-she;ShareholderPrecedenceRight"/>
   </owl:ObjectProperty>

   <owl:ObjectProperty rdf:about="&fibo-sec-eq-she;juniorEquityHasPriorityAsDefinedIn">
      <rdfs:label>junior equity has priority as defined in</rdfs:label>
      <rdfs:subPropertyOf rdf:resource="&fibo-sec-eq-she;hasPriorityAsDefinedIn"/>
      <rdfs:domain rdf:resource="&fibo-sec-eq-she;JuniorEquity"/>
      <rdfs:range rdf:resource="&fibo-sec-eq-she;JuniorEquityPriorityTermsSet"/>
   </owl:ObjectProperty>

   <owl:ObjectProperty rdf:about="&fibo-sec-eq-she;confersOwnershipOf">
      <rdfs:label>confers ownership of</rdfs:label>
      <rdfs:subPropertyOf rdf:resource="&fibo-sec-eq-eqi;confersOwnershipOfEquity"/>
      <rdfs:domain rdf:resource="&fibo-sec-eq-sh;OrdinaryShare"/>
      <rdfs:range rdf:resource="&fibo-sec-eq-she;JuniorEquity"/>
   </owl:ObjectProperty>

   <owl:ObjectProperty rdf:about="&fibo-sec-eq-she;otherSeniorityEquityHasPriorityAsDefinedIn">
      <rdfs:label>other seniority equity has priority as defined in</rdfs:label>
      <rdfs:subPropertyOf rdf:resource="&fibo-sec-eq-she;hasPriorityAsDefinedIn"/>
      <rdfs:domain rdf:resource="&fibo-sec-eq-she;OtherSeniorityEquity"/>
      <rdfs:range rdf:resource="&fibo-sec-eq-she;OtherEquityPriorityTermsSet"/>
   </owl:ObjectProperty>

   <owl:ObjectProperty rdf:about="&fibo-sec-eq-she;confersOwnershipOf.1">
      <rdfs:label>confers ownership of</rdfs:label>
      <rdfs:subPropertyOf rdf:resource="&fibo-sec-eq-eqi;confersOwnershipOfEquity"/>
      <rdfs:domain rdf:resource="&fibo-sec-eq-sh;PreferenceShare"/>
      <rdfs:range rdf:resource="&fibo-sec-eq-she;SeniorEquity"/>
   </owl:ObjectProperty>

   <owl:ObjectProperty rdf:about="&fibo-sec-eq-she;seniorEquityHasPriorityAsDefinedIn">
      <rdfs:label>senior equity has priority as defined in</rdfs:label>
      <rdfs:subPropertyOf rdf:resource="&fibo-sec-eq-she;hasPriorityAsDefinedIn"/>
      <rdfs:domain rdf:resource="&fibo-sec-eq-she;SeniorEquity"/>
      <rdfs:range rdf:resource="&fibo-sec-eq-she;SeniorEquityPriorityTermsSet"/>
   </owl:ObjectProperty>

   <owl:ObjectProperty rdf:about="&fibo-sec-eq-she;setOutIn">
      <rdfs:label>set out in</rdfs:label>
      <rdfs:subPropertyOf rdf:resource="&fibo-fnd-law-lcap;isConferredBy"/>
      <rdfs:domain rdf:resource="&fibo-sec-eq-she;ShareholderPrecedenceRight"/>
      <rdfs:range rdf:resource="&fibo-be-oac-exec;ArticlesOfIncorporation"/>
   </owl:ObjectProperty>

   <owl:ObjectProperty rdf:about="&fibo-sec-eq-she;hasPriorityAsDefinedIn">
      <rdfs:label>has priority as defined in</rdfs:label>
      <rdfs:domain rdf:resource="&fibo-sec-eq-eqi;ShareholderEquity"/>
      <rdfs:range rdf:resource="&fibo-sec-eq-she;EquityPriorityTermsSet"/>
   </owl:ObjectProperty>


  <!--
    ///////////////////////////////////////////////////////////////////////////////////////
    //
    // Data Properties
    //
    ///////////////////////////////////////////////////////////////////////////////////////
    -->


<owl:DatatypeProperty rdf:about="&fibo-sec-eq-she;juniorEquityPriority">
      <rdfs:label>junior equity priority</rdfs:label>
      <skos:definition>The seniority of the equity. This is the order of precedence in which holders of different classes of equity will have a call on the assets of the company in the event of it winding up. In the case of ordinary equity this is the lowest seniority i.e. it has the last call on the assets of the company.</skos:definition>
      <rdfs:range rdf:resource="&fibo-sec-eq-eqi;Seniority"/>
   </owl:DatatypeProperty>

   <owl:DatatypeProperty rdf:about="&fibo-sec-eq-she;otherEquityPriority">
      <rdfs:label>other equity priority</rdfs:label>
      <skos:definition>The seniority of the equity. This is the order of precedence in which holders of different classes of equity will have a call on the assets of the company in the event of it winding up. In this class of equity this is defined as being "Other" than highest or lowest, with the precise terms and order of precedence being defined in the priority terms.</skos:definition>
      <rdfs:range rdf:resource="&fibo-sec-eq-eqi;Seniority"/>
   </owl:DatatypeProperty>

   <owl:DatatypeProperty rdf:about="&fibo-sec-eq-she;seniorEquityPriority">
      <rdfs:label>senior equity priority</rdfs:label>
      <skos:definition>The seniority of the equity. This is the order of precedence in which holders of different classes of equity will have a call on the assets of the company in the event of it winding up. In this class of equity this is the highest in senioity.</skos:definition>
      <rdfs:range rdf:resource="&fibo-sec-eq-eqi;Seniority"/>
   </owl:DatatypeProperty>


  <!--
    ///////////////////////////////////////////////////////////////////////////////////////
    //
    // Annotation Properties
    //
    ///////////////////////////////////////////////////////////////////////////////////////
    -->



  <!--
    ///////////////////////////////////////////////////////////////////////////////////////
    //
    // Classes
    //
    ///////////////////////////////////////////////////////////////////////////////////////
    -->


<owl:Class rdf:about="&fibo-sec-eq-she;EquityPriorityTermsSet">
      <rdfs:label>equity priority terms set</rdfs:label>
      <skos:definition>Terms setting out the priority of a given class of Equity. These are the terms under which the holder of that class of equity has a call on the equity in the event of the issuing entity being wound up.</skos:definition>
      <rdfs:subClassOf rdf:resource="&fibo-sec-eq-sh;CompanyEquityTermsSet"/>
   </owl:Class>

   <owl:Class rdf:about="&fibo-sec-eq-she;JuniorEquity">
      <rdfs:label>junior equity</rdfs:label>
      <skos:definition>The most junior class of equity issued by a company. On the event of the company being wound up, holders of this class of equity have a call on the assets of the company only after the more senior classes of equity.</skos:definition>
      <rdfs:subClassOf rdf:resource="&fibo-sec-eq-eqi;ShareholderEquity"/>
   </owl:Class>

   <owl:Class rdf:about="&fibo-sec-eq-she;JuniorEquityPriorityTermsSet">
      <rdfs:label>junior equity priority terms set</rdfs:label>
      <skos:definition>The precise terms which define the seniority of this class of Equity. This is equity which has the lowest call on the assets of the issuer in the event of it being wound up, i.e. after Senior Equity and (if issued) other classes of equity.</skos:definition>
      <rdfs:subClassOf rdf:resource="&fibo-sec-eq-she;EquityPriorityTermsSet"/>
   </owl:Class>

   <owl:Class rdf:about="&fibo-sec-eq-she;OtherEquityPriorityTermsSet">
      <rdfs:label>other equity priority terms set</rdfs:label>
      <skos:definition>The precise terms which define the seniority of this class of Equity. These will set it apart from the highest of lowest seniority (senior or junior debt) and may be defined for more than one additional class of equity. These terms are defined by the issuer.</skos:definition>
   </owl:Class>

   <owl:Class rdf:about="&fibo-sec-eq-she;OtherSeniorityEquity">
      <rdfs:label>other seniority equity</rdfs:label>
      <skos:definition>Equity which is neither the most senior nor the most junior. The precise terms under which this equity is held, and the definition of the call on the assets of the company in the event of it winding up, will be defined by the issuing company and are not modelled here as they may vary from one company to another. There may be more than one class of such equity issued by a company.</skos:definition>
   </owl:Class>

   <owl:Class rdf:about="&fibo-sec-eq-she;SeniorEquity">
      <rdfs:label>senior equity</rdfs:label>
      <skos:definition>The most senior class of equity issued in the company. Holders of this class of equity will receive first call on the assets of the company in the event of it being wound up.</skos:definition>
   </owl:Class>

   <owl:Class rdf:about="&fibo-sec-eq-she;SeniorEquityPriorityTermsSet">
      <rdfs:label>senior equity priority terms set</rdfs:label>
      <skos:definition>The precise terms which define the seniority of this class of Equity. These terms set out that the holder has the first call among equity holders, on the assets of the issuing entity in the event of it being wound up, ahead of the holders of other classes of equity.</skos:definition>
   </owl:Class>

   <owl:Class rdf:about="&fibo-sec-eq-she;ShareholderPrecedenceRight">
      <rdfs:label>shareholder precedence right</rdfs:label>
      <skos:definition>The rights of shareholderes in respect of the assets of the limited company in which they hold those shares, in the event of that company being wound up.</skos:definition>
      <rdfs:subClassOf rdf:resource="&fibo-sec-eq-sh;PrecedenceRight"/>
   </owl:Class>


  <!--
    ///////////////////////////////////////////////////////////////////////////////////////
    //
    // Individuals
    //
    ///////////////////////////////////////////////////////////////////////////////////////
    -->


</rdf:RDF>