<?xml version="1.0" encoding="UTF-8"?>
<!DOCTYPE rdf:RDF [
	<!ENTITY dct "http://purl.org/dc/terms/">
	<!ENTITY fibo-fbc-fct-eufse "https://spec.edmcouncil.org/fibo/FBC/FunctionalEntities/EuropeanEntities/EUFinancialServicesEntities/">
	<!ENTITY fibo-fbc-fct-fse "https://spec.edmcouncil.org/fibo/FBC/FunctionalEntities/FinancialServicesEntities/">
	<!ENTITY fibo-fnd-pty-rl "https://spec.edmcouncil.org/fibo/FND/Parties/Roles/">
	<!ENTITY fibo-fnd-rel-rel "https://spec.edmcouncil.org/fibo/FND/Relations/Relations/">
	<!ENTITY fibo-fnd-utl-av "https://spec.edmcouncil.org/fibo/FND/Utilities/AnnotationVocabulary/">
	<!ENTITY owl "http://www.w3.org/2002/07/owl#">
	<!ENTITY rdf "http://www.w3.org/1999/02/22-rdf-syntax-ns#">
	<!ENTITY rdfs "http://www.w3.org/2000/01/rdf-schema#">
	<!ENTITY skos "http://www.w3.org/2004/02/skos/core#">
	<!ENTITY sm "http://www.omg.org/techprocess/ab/SpecificationMetadata/">
	<!ENTITY xsd "http://www.w3.org/2001/XMLSchema#">
]>
<rdf:RDF xml:base="https://spec.edmcouncil.org/fibo/FBC/FunctionalEntities/EuropeanEntities/EUFinancialServicesEntities/"
	xmlns:dct="http://purl.org/dc/terms/"
	xmlns:fibo-fbc-fct-eufse="https://spec.edmcouncil.org/fibo/FBC/FunctionalEntities/EuropeanEntities/EUFinancialServicesEntities/"
	xmlns:fibo-fbc-fct-fse="https://spec.edmcouncil.org/fibo/FBC/FunctionalEntities/FinancialServicesEntities/"
	xmlns:fibo-fnd-pty-rl="https://spec.edmcouncil.org/fibo/FND/Parties/Roles/"
	xmlns:fibo-fnd-rel-rel="https://spec.edmcouncil.org/fibo/FND/Relations/Relations/"
	xmlns:fibo-fnd-utl-av="https://spec.edmcouncil.org/fibo/FND/Utilities/AnnotationVocabulary/"
	xmlns:owl="http://www.w3.org/2002/07/owl#"
	xmlns:rdf="http://www.w3.org/1999/02/22-rdf-syntax-ns#"
	xmlns:rdfs="http://www.w3.org/2000/01/rdf-schema#"
	xmlns:skos="http://www.w3.org/2004/02/skos/core#"
	xmlns:sm="http://www.omg.org/techprocess/ab/SpecificationMetadata/"
	xmlns:xsd="http://www.w3.org/2001/XMLSchema#">
	
	<owl:Ontology rdf:about="https://spec.edmcouncil.org/fibo/FBC/FunctionalEntities/EuropeanEntities/EUFinancialServicesEntities/">
		<rdfs:label>European Financial Services Entities Ontology</rdfs:label>
		<dct:license rdf:resource="&sm;MITLicense"/>
		<sm:contentLanguage rdf:datatype="&xsd;anyURI">http://www.omg.org/spec/ODM/</sm:contentLanguage>
		<sm:contentLanguage rdf:datatype="&xsd;anyURI">http://www.w3.org/standards/techs/owl#w3c_all</sm:contentLanguage>
		<sm:copyright>Copyright (c) 2017 EDM Council, Inc.
Copyright (c) 2017 Object Management Group, Inc.</sm:copyright>
		<sm:dependsOn rdf:datatype="&xsd;anyURI">https://spec.edmcouncil.org/fibo/BE/</sm:dependsOn>
		<sm:dependsOn rdf:datatype="&xsd;anyURI">https://spec.edmcouncil.org/fibo/FBC/FunctionalEntities/FinancialServicesEntities/</sm:dependsOn>
		<sm:dependsOn rdf:datatype="&xsd;anyURI">https://spec.edmcouncil.org/fibo/FBC/ProductsAndServices/FinancialProductsAndServices/</sm:dependsOn>
		<sm:dependsOn rdf:datatype="&xsd;anyURI">https://spec.edmcouncil.org/fibo/FND/</sm:dependsOn>
		<sm:fileAbbreviation>fibo-fbc-fct-eufse</sm:fileAbbreviation>
		<sm:fileAbstract>This ontology extends the primary financial services entities ontology in FBC with additional kinds of entities that that provide services in Europe, across national boundaries, such as European market data providers, organizations that provide exchanges in multiple countries, organizations that support the European Union, and so forth.</sm:fileAbstract>
		<sm:filename>EUFinancialServicesEntities.rdf</sm:filename>
		<rdfs:seeAlso rdf:resource="https://spec.edmcouncil.org/fibo/AboutTheEDMC-FIBOFamily/"/>
		<rdfs:seeAlso rdf:resource="https://spec.edmcouncil.org/fibo/FBC/AboutFBC/"/>
		<rdfs:seeAlso rdf:resource="https://spec.edmcouncil.org/fibo/FBC/FunctionalEntities/AboutFBCFunctionalEntities/"/>
		<owl:imports rdf:resource="https://spec.edmcouncil.org/fibo/FBC/FunctionalEntities/FinancialServicesEntities/"/>
		<owl:imports rdf:resource="https://spec.edmcouncil.org/fibo/FBC/ProductsAndServices/FinancialProductsAndServices/"/>
		<owl:imports rdf:resource="https://spec.edmcouncil.org/fibo/FND/Parties/Roles/"/>
		<owl:imports rdf:resource="https://spec.edmcouncil.org/fibo/FND/Relations/Relations/"/>
		<owl:imports rdf:resource="https://spec.edmcouncil.org/fibo/FND/Utilities/AnnotationVocabulary/"/>
		<owl:versionIRI rdf:resource="https://spec.edmcouncil.org/fibo/FBC/20170801/FunctionalEntities/EuropeanEntities/EUFinancialServicesEntities/"/>
		<skos:changeNote>The https://spec.edmcouncil.org/fibo/FBC/20170801/FunctionalEntities/EuropeanEntities/EUFinancialServicesEntities.rdf version of this ontology was added per the issue resolutions identified in the FIBO FBC 1.1 RTF report.</skos:changeNote>
		<fibo-fnd-utl-av:hasMaturityLevel rdf:resource="&fibo-fnd-utl-av;Release"/>
	</owl:Ontology>
	
	<owl:Class rdf:about="&fibo-fbc-fct-eufse;CRDCreditInstitution">
		<rdfs:subClassOf rdf:resource="&fibo-fbc-fct-eufse;CreditInstitution"/>
		<rdfs:label>CRD credit institution</rdfs:label>
		<owl:disjointWith rdf:resource="&fibo-fbc-fct-eufse;EuropeanEconomicAreaBranch"/>
		<owl:disjointWith rdf:resource="&fibo-fbc-fct-eufse;NonEuropeanEconomicAreaBranch"/>
		<skos:definition>an undertaking whose business is to receive deposits or other repayable funds from the public and to grant credits for its own account as defined by the European Banking Authority (EBA)</skos:definition>
		<fibo-fnd-utl-av:definitionOrigin rdf:datatype="&xsd;anyURI">http://www.eba.europa.eu/risk-analysis-and-data/credit-institutions-register</fibo-fnd-utl-av:definitionOrigin>
	</owl:Class>
	
	<owl:Class rdf:about="&fibo-fbc-fct-eufse;CreditInstitution">
		<rdfs:subClassOf rdf:resource="&fibo-fbc-fct-eufse;CreditInstitutionOrInvestmentFirm"/>
		<rdfs:label>credit institution</rdfs:label>
		<skos:definition>an undertaking the business of which is to take deposits or other repayable funds from the public and to grant credits for its own account, and to which authorisation has been granted to operate within the European Union and European Economic Area countries (EEA)</skos:definition>
		<fibo-fnd-utl-av:adaptedFrom rdf:datatype="&xsd;anyURI">http://eur-lex.europa.eu/legal-content/EN/TXT/PDF/?uri=CELEX:32013R0575&amp;from=EN#page=18</fibo-fnd-utl-av:adaptedFrom>
		<fibo-fnd-utl-av:adaptedFrom rdf:datatype="&xsd;anyURI">http://www.eba.europa.eu/risk-analysis-and-data/credit-institutions-register</fibo-fnd-utl-av:adaptedFrom>
	</owl:Class>
	
	<owl:Class rdf:about="&fibo-fbc-fct-eufse;CreditInstitutionOrInvestmentFirm">
		<rdfs:subClassOf rdf:resource="&fibo-fbc-fct-fse;FinancialInstitution"/>
		<rdfs:label>credit institution or investment firm</rdfs:label>
		<skos:definition>a European financial institution that is a credit institution or an investment firm as defined by the European Banking Authority (EBA)</skos:definition>
		<fibo-fnd-utl-av:adaptedFrom rdf:datatype="&xsd;anyURI">http://eur-lex.europa.eu/legal-content/EN/TXT/PDF/?uri=CELEX:32013R0575&amp;from=EN#page=18</fibo-fnd-utl-av:adaptedFrom>
	</owl:Class>
	
	<owl:Class rdf:about="&fibo-fbc-fct-eufse;EuropeanEconomicAreaBranch">
		<rdfs:subClassOf rdf:resource="&fibo-fbc-fct-eufse;CreditInstitution"/>
		<rdfs:label>European Economic Area branch</rdfs:label>
		<owl:disjointWith rdf:resource="&fibo-fbc-fct-eufse;NonEuropeanEconomicAreaBranch"/>
		<skos:definition>a branch of a credit institution authorised in another European Economic Area (EEA) country that has the right to passport its activities</skos:definition>
		<fibo-fnd-utl-av:definitionOrigin rdf:datatype="&xsd;anyURI">http://www.eba.europa.eu/risk-analysis-and-data/credit-institutions-register</fibo-fnd-utl-av:definitionOrigin>
		<fibo-fnd-utl-av:synonym>EEA branch</fibo-fnd-utl-av:synonym>
	</owl:Class>
	
	<owl:Class rdf:about="&fibo-fbc-fct-eufse;InvestmentFirm">
		<rdfs:subClassOf rdf:resource="&fibo-fbc-fct-eufse;CreditInstitutionOrInvestmentFirm"/>
		<rdfs:subClassOf>
			<owl:Class>
				<owl:unionOf rdf:parseType="Collection">
					<rdf:Description rdf:about="&fibo-fbc-fct-fse;BrokerageFirm">
					</rdf:Description>
					<rdf:Description rdf:about="&fibo-fbc-fct-fse;InvestmentCompany">
					</rdf:Description>
					<owl:Restriction>
						<owl:onProperty rdf:resource="&fibo-fnd-pty-rl;isPlayedBy"/>
						<owl:someValuesFrom>
							<owl:Restriction>
								<owl:onProperty rdf:resource="&fibo-fnd-rel-rel;provides"/>
								<owl:someValuesFrom rdf:resource="&fibo-fbc-fct-fse;InvestmentService"/>
							</owl:Restriction>
						</owl:someValuesFrom>
					</owl:Restriction>
				</owl:unionOf>
			</owl:Class>
		</rdfs:subClassOf>
		<rdfs:label>investment firm</rdfs:label>
		<owl:disjointWith rdf:resource="&fibo-fbc-fct-eufse;CreditInstitution"/>
		<owl:disjointWith rdf:resource="&fibo-fbc-fct-eufse;LocalFirm"/>
		<skos:definition>any legal person whose regular occupation or business is the provision of one or more investment services to third parties and/or the performance of one or more investment activities on a professional basis</skos:definition>
		<fibo-fnd-utl-av:adaptedFrom rdf:datatype="&xsd;anyURI">http://eur-lex.europa.eu/legal-content/EN/TXT/PDF/?uri=CELEX:32004L0039&amp;from=en#page=9</fibo-fnd-utl-av:adaptedFrom>
	</owl:Class>
	
	<owl:Class rdf:about="&fibo-fbc-fct-eufse;LocalFirm">
		<rdfs:subClassOf rdf:resource="&fibo-fbc-fct-eufse;CreditInstitutionOrInvestmentFirm"/>
		<rdfs:subClassOf rdf:resource="&fibo-fbc-fct-fse;BrokerageFirm"/>
		<rdfs:label>local firm</rdfs:label>
		<skos:definition>a firm dealing for its own account on markets in financial futures or options or other derivatives and on cash markets for the sole purpose of hedging positions on derivatives markets, or dealing for the accounts of other members of those markets and being guaranteed by clearing members of the same markets, where responsibility for ensuring the performance of contracts entered into by such a firm is assumed by clearing members of the same markets</skos:definition>
		<fibo-fnd-utl-av:adaptedFrom rdf:datatype="&xsd;anyURI">http://eur-lex.europa.eu/legal-content/EN/TXT/PDF/?uri=CELEX:32013R0575&amp;from=EN#page=18</fibo-fnd-utl-av:adaptedFrom>
	</owl:Class>
	
	<owl:Class rdf:about="&fibo-fbc-fct-eufse;NonEuropeanEconomicAreaBranch">
		<rdfs:subClassOf rdf:resource="&fibo-fbc-fct-eufse;CreditInstitution"/>
		<rdfs:label>non European Economic Area branch</rdfs:label>
		<skos:definition>a branch of a credit institution whose Head Office is in a third country</skos:definition>
		<fibo-fnd-utl-av:definitionOrigin rdf:datatype="&xsd;anyURI">http://www.eba.europa.eu/risk-analysis-and-data/credit-institutions-register</fibo-fnd-utl-av:definitionOrigin>
		<fibo-fnd-utl-av:synonym>non-EEA branch</fibo-fnd-utl-av:synonym>
	</owl:Class>
	
	<owl:Class rdf:about="&fibo-fbc-fct-eufse;PaymentInstitution">
		<rdfs:subClassOf rdf:resource="&fibo-fbc-fct-eufse;CreditInstitutionOrInvestmentFirm"/>
		<rdfs:subClassOf>
			<owl:Restriction>
				<owl:onProperty rdf:resource="&fibo-fnd-pty-rl;isPlayedBy"/>
				<owl:someValuesFrom>
					<owl:Restriction>
						<owl:onProperty rdf:resource="&fibo-fnd-rel-rel;provides"/>
						<owl:someValuesFrom rdf:resource="&fibo-fbc-fct-fse;PaymentService"/>
					</owl:Restriction>
				</owl:someValuesFrom>
			</owl:Restriction>
		</rdfs:subClassOf>
		<rdfs:label>payment institution</rdfs:label>
		<skos:definition>a legal person that has been granted authorisation in accordance with Article 10 to provide and execute payment services throughout the European community</skos:definition>
		<fibo-fnd-utl-av:adaptedFrom rdf:datatype="&xsd;anyURI">http://eur-lex.europa.eu/legal-content/EN/TXT/PDF/?uri=CELEX:32007L0064&amp;from=EN#page=18</fibo-fnd-utl-av:adaptedFrom>
	</owl:Class>

</rdf:RDF>