<?xml version="1.0" encoding="UTF-8"?>
<!DOCTYPE rdf:RDF [
	<!ENTITY cmns-av "https://www.omg.org/spec/Commons/AnnotationVocabulary/">
	<!ENTITY cmns-col "https://www.omg.org/spec/Commons/Collections/">
	<!ENTITY cmns-dt "https://www.omg.org/spec/Commons/DatesAndTimes/">
	<!ENTITY cmns-id "https://www.omg.org/spec/Commons/Identifiers/">
	<!ENTITY cmns-rlcmp "https://www.omg.org/spec/Commons/RolesAndCompositions/">
	<!ENTITY dct "http://purl.org/dc/terms/">
	<!ENTITY fibo-be-ge-ge "https://spec.edmcouncil.org/fibo/ontology/BE/GovernmentEntities/GovernmentEntities/">
	<!ENTITY fibo-be-le-fbo "https://spec.edmcouncil.org/fibo/ontology/BE/LegalEntities/FormalBusinessOrganizations/">
	<!ENTITY fibo-be-le-lei "https://spec.edmcouncil.org/fibo/ontology/BE/LegalEntities/LEIEntities/">
	<!ENTITY fibo-fbc-fct-bci "https://spec.edmcouncil.org/fibo/ontology/FBC/FunctionalEntities/BusinessCentersIndividuals/">
	<!ENTITY fibo-fbc-fct-breg "https://spec.edmcouncil.org/fibo/ontology/FBC/FunctionalEntities/BusinessRegistries/">
	<!ENTITY fibo-fbc-fct-fse "https://spec.edmcouncil.org/fibo/ontology/FBC/FunctionalEntities/FinancialServicesEntities/">
	<!ENTITY fibo-fbc-fct-ireg "https://spec.edmcouncil.org/fibo/ontology/FBC/FunctionalEntities/InternationalRegistriesAndAuthorities/">
	<!ENTITY fibo-fbc-fct-mkt "https://spec.edmcouncil.org/fibo/ontology/FBC/FunctionalEntities/Markets/">
	<!ENTITY fibo-fbc-fct-ra "https://spec.edmcouncil.org/fibo/ontology/FBC/FunctionalEntities/RegistrationAuthorities/">
	<!ENTITY fibo-fbc-fct-rga "https://spec.edmcouncil.org/fibo/ontology/FBC/FunctionalEntities/RegulatoryAgencies/">
	<!ENTITY fibo-fbc-pas-fpas "https://spec.edmcouncil.org/fibo/ontology/FBC/ProductsAndServices/FinancialProductsAndServices/">
	<!ENTITY fibo-fnd-plc-adr "https://spec.edmcouncil.org/fibo/ontology/FND/Places/Addresses/">
	<!ENTITY fibo-fnd-plc-loc "https://spec.edmcouncil.org/fibo/ontology/FND/Places/Locations/">
	<!ENTITY fibo-fnd-plc-vrt "https://spec.edmcouncil.org/fibo/ontology/FND/Places/VirtualPlaces/">
	<!ENTITY fibo-fnd-rel-rel "https://spec.edmcouncil.org/fibo/ontology/FND/Relations/Relations/">
	<!ENTITY fibo-fnd-utl-av "https://spec.edmcouncil.org/fibo/ontology/FND/Utilities/AnnotationVocabulary/">
	<!ENTITY lcc-3166-1 "https://www.omg.org/spec/LCC/Countries/ISO3166-1-CountryCodes/">
	<!ENTITY owl "http://www.w3.org/2002/07/owl#">
	<!ENTITY rdf "http://www.w3.org/1999/02/22-rdf-syntax-ns#">
	<!ENTITY rdfs "http://www.w3.org/2000/01/rdf-schema#">
	<!ENTITY skos "http://www.w3.org/2004/02/skos/core#">
	<!ENTITY xsd "http://www.w3.org/2001/XMLSchema#">
]>
<rdf:RDF xml:base="https://spec.edmcouncil.org/fibo/ontology/FBC/FunctionalEntities/InternationalRegistriesAndAuthorities/"
	xmlns:cmns-av="https://www.omg.org/spec/Commons/AnnotationVocabulary/"
	xmlns:cmns-col="https://www.omg.org/spec/Commons/Collections/"
	xmlns:cmns-dt="https://www.omg.org/spec/Commons/DatesAndTimes/"
	xmlns:cmns-id="https://www.omg.org/spec/Commons/Identifiers/"
	xmlns:cmns-rlcmp="https://www.omg.org/spec/Commons/RolesAndCompositions/"
	xmlns:dct="http://purl.org/dc/terms/"
	xmlns:fibo-be-ge-ge="https://spec.edmcouncil.org/fibo/ontology/BE/GovernmentEntities/GovernmentEntities/"
	xmlns:fibo-be-le-fbo="https://spec.edmcouncil.org/fibo/ontology/BE/LegalEntities/FormalBusinessOrganizations/"
	xmlns:fibo-be-le-lei="https://spec.edmcouncil.org/fibo/ontology/BE/LegalEntities/LEIEntities/"
	xmlns:fibo-fbc-fct-bci="https://spec.edmcouncil.org/fibo/ontology/FBC/FunctionalEntities/BusinessCentersIndividuals/"
	xmlns:fibo-fbc-fct-breg="https://spec.edmcouncil.org/fibo/ontology/FBC/FunctionalEntities/BusinessRegistries/"
	xmlns:fibo-fbc-fct-fse="https://spec.edmcouncil.org/fibo/ontology/FBC/FunctionalEntities/FinancialServicesEntities/"
	xmlns:fibo-fbc-fct-ireg="https://spec.edmcouncil.org/fibo/ontology/FBC/FunctionalEntities/InternationalRegistriesAndAuthorities/"
	xmlns:fibo-fbc-fct-mkt="https://spec.edmcouncil.org/fibo/ontology/FBC/FunctionalEntities/Markets/"
	xmlns:fibo-fbc-fct-ra="https://spec.edmcouncil.org/fibo/ontology/FBC/FunctionalEntities/RegistrationAuthorities/"
	xmlns:fibo-fbc-fct-rga="https://spec.edmcouncil.org/fibo/ontology/FBC/FunctionalEntities/RegulatoryAgencies/"
	xmlns:fibo-fbc-pas-fpas="https://spec.edmcouncil.org/fibo/ontology/FBC/ProductsAndServices/FinancialProductsAndServices/"
	xmlns:fibo-fnd-plc-adr="https://spec.edmcouncil.org/fibo/ontology/FND/Places/Addresses/"
	xmlns:fibo-fnd-plc-loc="https://spec.edmcouncil.org/fibo/ontology/FND/Places/Locations/"
	xmlns:fibo-fnd-plc-vrt="https://spec.edmcouncil.org/fibo/ontology/FND/Places/VirtualPlaces/"
	xmlns:fibo-fnd-rel-rel="https://spec.edmcouncil.org/fibo/ontology/FND/Relations/Relations/"
	xmlns:fibo-fnd-utl-av="https://spec.edmcouncil.org/fibo/ontology/FND/Utilities/AnnotationVocabulary/"
	xmlns:lcc-3166-1="https://www.omg.org/spec/LCC/Countries/ISO3166-1-CountryCodes/"
	xmlns:owl="http://www.w3.org/2002/07/owl#"
	xmlns:rdf="http://www.w3.org/1999/02/22-rdf-syntax-ns#"
	xmlns:rdfs="http://www.w3.org/2000/01/rdf-schema#"
	xmlns:skos="http://www.w3.org/2004/02/skos/core#"
	xmlns:xsd="http://www.w3.org/2001/XMLSchema#">
	
	<owl:Ontology rdf:about="https://spec.edmcouncil.org/fibo/ontology/FBC/FunctionalEntities/InternationalRegistriesAndAuthorities/">
		<rdfs:label>International Registries and Authorities Ontology</rdfs:label>
		<dct:abstract>This ontology extends the Business Registries ontology to define commonly referenced international registration authorities and related registry details, where the multi-national responsibilities for registering and/or managing various identifiers needed in banking applications occur, such as SWIFT. These individuals and in some cases, such as registry entries, are managed independently to reduce the import footprint for applications that do not require them, in other words, to support modularity needs of FIBO users.</dct:abstract>
		<dct:license rdf:datatype="&xsd;anyURI">https://opensource.org/licenses/MIT</dct:license>
		<owl:imports rdf:resource="https://spec.edmcouncil.org/fibo/ontology/BE/GovernmentEntities/GovernmentEntities/"/>
		<owl:imports rdf:resource="https://spec.edmcouncil.org/fibo/ontology/BE/LegalEntities/FormalBusinessOrganizations/"/>
		<owl:imports rdf:resource="https://spec.edmcouncil.org/fibo/ontology/BE/LegalEntities/LEIEntities/"/>
		<owl:imports rdf:resource="https://spec.edmcouncil.org/fibo/ontology/FBC/FunctionalEntities/BusinessRegistries/"/>
		<owl:imports rdf:resource="https://spec.edmcouncil.org/fibo/ontology/FBC/FunctionalEntities/FinancialServicesEntities/"/>
		<owl:imports rdf:resource="https://spec.edmcouncil.org/fibo/ontology/FBC/FunctionalEntities/Markets/"/>
		<owl:imports rdf:resource="https://spec.edmcouncil.org/fibo/ontology/FBC/FunctionalEntities/RegistrationAuthorities/"/>
		<owl:imports rdf:resource="https://spec.edmcouncil.org/fibo/ontology/FBC/FunctionalEntities/RegulatoryAgencies/"/>
		<owl:imports rdf:resource="https://spec.edmcouncil.org/fibo/ontology/FBC/ProductsAndServices/FinancialProductsAndServices/"/>
		<owl:imports rdf:resource="https://spec.edmcouncil.org/fibo/ontology/FND/Places/Addresses/"/>
		<owl:imports rdf:resource="https://spec.edmcouncil.org/fibo/ontology/FND/Places/Locations/"/>
		<owl:imports rdf:resource="https://spec.edmcouncil.org/fibo/ontology/FND/Places/VirtualPlaces/"/>
		<owl:imports rdf:resource="https://spec.edmcouncil.org/fibo/ontology/FND/Relations/Relations/"/>
		<owl:imports rdf:resource="https://spec.edmcouncil.org/fibo/ontology/FND/Utilities/AnnotationVocabulary/"/>
		<owl:imports rdf:resource="https://www.omg.org/spec/Commons/AnnotationVocabulary/"/>
		<owl:imports rdf:resource="https://www.omg.org/spec/Commons/Collections/"/>
		<owl:imports rdf:resource="https://www.omg.org/spec/Commons/DatesAndTimes/"/>
		<owl:imports rdf:resource="https://www.omg.org/spec/Commons/Identifiers/"/>
		<owl:imports rdf:resource="https://www.omg.org/spec/Commons/RolesAndCompositions/"/>
		<owl:imports rdf:resource="https://www.omg.org/spec/LCC/Countries/ISO3166-1-CountryCodes/"/>
		<owl:versionIRI rdf:resource="https://spec.edmcouncil.org/fibo/ontology/FBC/20240101/FunctionalEntities/InternationalRegistriesAndAuthorities/"/>
		<skos:changeNote>The https://spec.edmcouncil.org/fibo/ontology/FBC/20200301/FunctionalEntities/InternationalRegistriesAndAuthorities.rdf version of this ontology was revised to add details for the Global LEI Foundation and fix spelling errors.</skos:changeNote>
		<skos:changeNote>The https://spec.edmcouncil.org/fibo/ontology/FBC/20211201/FunctionalEntities/InternationalRegistriesAndAuthorities.rdf version of this ontology was revised to address text formatting issues uncovered via hygiene testing.</skos:changeNote>
		<skos:changeNote>The https://spec.edmcouncil.org/fibo/ontology/FBC/20220801/FunctionalEntities/InternationalRegistriesAndAuthorities.rdf version of the ontology was modified to use the Commons Ontology Library (Commons) Annotation Vocabulary rather than the OMG&apos;s Specification Metadata vocabulary.</skos:changeNote>
		<skos:changeNote>The https://spec.edmcouncil.org/fibo/ontology/FBC/20230101/FunctionalEntities/InternationalRegistriesAndAuthorities.rdf version of this ontology was modified to use the Commons Ontology Library (Commons) rather than the OMG&apos;s Languages, Countries and Codes (LCC) and to eliminate redundancies in FIBO as appropriate.</skos:changeNote>
		<skos:changeNote>The https://spec.edmcouncil.org/fibo/ontology/FBC/20230301/FunctionalEntities/InternationalRegistriesAndAuthorities.rdf version of this ontology was modified to replace content that is now available in the OMG Commons Ontology Library (Commons) v1.1 (FND-380).</skos:changeNote>
		<fibo-fnd-utl-av:hasMaturityLevel rdf:resource="&fibo-fnd-utl-av;Release"/>
		<cmns-av:copyright>Copyright (c) 2015-2024 EDM Council, Inc.</cmns-av:copyright>
		<cmns-av:copyright>Copyright (c) 2015-2024 Object Management Group, Inc.</cmns-av:copyright>
	</owl:Ontology>
	
	<owl:NamedIndividual rdf:about="https://rdf.gleif.org/L1/L-506700GE1G29325QX363-LEI">
		<rdf:type rdf:resource="&fibo-be-le-lei;LegalEntityIdentifier"/>
		<rdfs:label>Global Legal Entity Identifier Foundation legal entity identifier</rdfs:label>
		<skos:definition>identifier and link to the official legal entity identifier registry entry for the Global Legal Entity Identifier Foundation as published in the Global LEI Index</skos:definition>
		<fibo-fbc-fct-ra:isRegisteredIn rdf:resource="&fibo-fbc-fct-ireg;GlobalLEIIndex"/>
		<fibo-fnd-rel-rel:hasTag>506700GE1G29325QX363</fibo-fnd-rel-rel:hasTag>
		<cmns-id:identifies rdf:resource="&fibo-fbc-fct-ireg;GlobalLegalEntityIdentifierFoundation"/>
	</owl:NamedIndividual>
	
	<owl:NamedIndividual rdf:about="https://rdf.gleif.org/L1/L-HB7FFAZI0OMZ8PP8OE26-LEI">
		<rdf:type rdf:resource="&fibo-be-le-lei;LegalEntityIdentifier"/>
		<rdfs:label>Society for Worldwide Interbank Financial Telecommunication (SWIFT) legal entity identifier</rdfs:label>
		<skos:definition>identifier and link to the official legal entity identifier registry entry for the Society for Worldwide Interbank Financial Telecommunication (SWIFT)</skos:definition>
		<fibo-fbc-fct-ra:isRegisteredIn rdf:resource="&fibo-fbc-fct-ireg;GlobalLEIIndex"/>
		<fibo-fnd-rel-rel:hasTag>HB7FFAZI0OMZ8PP8OE26</fibo-fnd-rel-rel:hasTag>
		<cmns-id:identifies rdf:resource="&fibo-fbc-fct-ireg;SocietyForWorldwideInterbankFinancialTelecommunication"/>
	</owl:NamedIndividual>
	
	<owl:NamedIndividual rdf:about="https://rdf.gleif.org/L1/L-UXIATLMNPCXXT5KR1S08-LEI">
		<rdf:type rdf:resource="&fibo-be-le-lei;LegalEntityIdentifier"/>
		<rdfs:label>Bank for International Settlements legal entity identifier</rdfs:label>
		<skos:definition>identifier and link to the official legal entity identifier registry entry for the Bank for International Settlements</skos:definition>
		<fibo-fbc-fct-ra:isRegisteredIn rdf:resource="&fibo-fbc-fct-ireg;GlobalLEIIndex"/>
		<fibo-fnd-rel-rel:hasTag>UXIATLMNPCXXT5KR1S08</fibo-fnd-rel-rel:hasTag>
		<cmns-id:identifies rdf:resource="&fibo-fbc-fct-ireg;BankForInternationalSettlements"/>
	</owl:NamedIndividual>
	
	<owl:NamedIndividual rdf:about="&fibo-fbc-fct-ireg;BankForInternationalSettlements">
		<rdf:type rdf:resource="&fibo-be-ge-ge;Instrumentality"/>
		<rdfs:label xml:lang="en">Bank for International Settlements</rdfs:label>
		<rdfs:label xml:lang="de">Bank für Internationalen Zahlungsausgleich</rdfs:label>
		<rdfs:label xml:lang="fr">Banque Des Reglements Internationaux</rdfs:label>
		<skos:definition>international financial organization that serves central banks in their pursuit of monetary and financial stability, helping to foster international cooperation in those areas and acting as a bank for central banks</skos:definition>
		<fibo-be-le-fbo:hasHeadquartersAddress rdf:resource="&fibo-fbc-fct-ireg;BankForInternationalSettlementsAddress"/>
		<fibo-be-le-lei:hasLegalAddress rdf:resource="&fibo-fbc-fct-ireg;BankForInternationalSettlementsAddress"/>
		<fibo-fnd-plc-vrt:hasWebsite rdf:datatype="&xsd;anyURI">https://www.bis.org/</fibo-fnd-plc-vrt:hasWebsite>
		<fibo-fnd-rel-rel:hasLegalName xml:lang="de">Bank für Internationalen Zahlungsausgleich</fibo-fnd-rel-rel:hasLegalName>
		<cmns-av:abbreviation>BIS</cmns-av:abbreviation>
		<cmns-av:adaptedFrom>Office of Financial Research (OFR) Annual Report, 2012, Glossary</cmns-av:adaptedFrom>
		<cmns-av:explanatoryNote>Established in 1930, the BIS is owned by 63 central banks, representing countries from around the world that together account for about 95 percent of world GDP. Its head office is in Basel, Switzerland and it has two representative offices: in Hong Kong SAR and in Mexico City, as well as Innovation Hub Centres around the world.</cmns-av:explanatoryNote>
	</owl:NamedIndividual>
	
	<owl:NamedIndividual rdf:about="&fibo-fbc-fct-ireg;BankForInternationalSettlementsAddress">
		<rdf:type rdf:resource="&fibo-fnd-plc-adr;ConventionalStreetAddress"/>
		<rdfs:label>Bank for International Settlements address</rdfs:label>
		<skos:definition>Tower building address for the Bank for International Settlements (BIS)</skos:definition>
		<fibo-fnd-plc-adr:hasAddressLine1>Centralbahnplatz 2</fibo-fnd-plc-adr:hasAddressLine1>
		<fibo-fnd-plc-adr:hasPostalCode>4051</fibo-fnd-plc-adr:hasPostalCode>
		<fibo-fnd-plc-loc:hasCountry rdf:resource="&lcc-3166-1;Switzerland"/>
		<fibo-fnd-plc-loc:hasMunicipality rdf:resource="&fibo-fbc-fct-bci;Basel"/>
	</owl:NamedIndividual>
	
	<owl:NamedIndividual rdf:about="&fibo-fbc-fct-ireg;BankForInternationalSettlementsAsBankingServicesProvider">
		<rdf:type rdf:resource="&fibo-fbc-fct-fse;Bank"/>
		<rdfs:label xml:lang="en">Bank for International Settlements as banking services provider</rdfs:label>
		<rdfs:seeAlso rdf:resource="https://www.bis.org/"/>
		<skos:definition>Bank for International Settlements role as a banking services provider to central banks and other monetary authorities</skos:definition>
		<fibo-fbc-fct-fse:hasDateEstablished rdf:resource="&fibo-fbc-fct-ireg;BankForInternationalSettlementsDateEstablished"/>
		<cmns-av:adaptedFrom>Office of Financial Research (OFR) Annual Report, 2012, Glossary</cmns-av:adaptedFrom>
		<cmns-av:explanatoryNote>The Bank for International Settlements offers a wide range of financial services specifically designed to assist central banks and other official monetary institutions in the management of their foreign exchange reserves. BIS facilitates international financial cooperation and endeavors to make monetary policy more predictable and transparent. Its customers are central banks and international organizations; they do not accept deposits from, or provide financial services to, private individuals or corporate entities.</cmns-av:explanatoryNote>
		<cmns-rlcmp:isPlayedBy rdf:resource="&fibo-fbc-fct-ireg;BankForInternationalSettlements"/>
	</owl:NamedIndividual>
	
	<owl:NamedIndividual rdf:about="&fibo-fbc-fct-ireg;BankForInternationalSettlementsDateEstablished">
		<rdf:type rdf:resource="&cmns-dt;ExplicitDate"/>
		<rdfs:label>Bank for International Settlements date established</rdfs:label>
		<skos:definition>date that Bank for International Settlements was established to offer financial services to BIS member central banks</skos:definition>
		<cmns-dt:hasDateValue>1930-05-01</cmns-dt:hasDateValue>
	</owl:NamedIndividual>
	
	<owl:NamedIndividual rdf:about="&fibo-fbc-fct-ireg;BankForInternationalSettlementsLegalEntityIdentifierRegistryEntry">
		<rdf:type rdf:resource="&fibo-fbc-fct-breg;LegalEntityIdentifierRegistryEntry"/>
		<rdfs:label>Bank for International Settlements legal entity identifier registry entry</rdfs:label>
		<skos:definition>Global LEI Index registry entry for Bank for International Settlements (BIS)</skos:definition>
		<fibo-fbc-fct-breg:hasInitialRegistrationDate rdf:datatype="&xsd;dateTime">2012-06-06T08:55:00-07:00</fibo-fbc-fct-breg:hasInitialRegistrationDate>
		<fibo-fbc-fct-breg:hasRegistrationRevisionDate rdf:datatype="&xsd;dateTime">2021-06-29T14:31:00-07:00</fibo-fbc-fct-breg:hasRegistrationRevisionDate>
		<fibo-fbc-fct-breg:hasRegistrationStatus rdf:resource="&fibo-fbc-fct-breg;IssuedStatus"/>
		<fibo-fbc-fct-breg:hasRenewalDate rdf:datatype="&xsd;dateTime">2022-06-25T07:42:00-07:00</fibo-fbc-fct-breg:hasRenewalDate>
		<fibo-fbc-fct-breg:hasValidationLevel rdf:resource="&fibo-fbc-fct-breg;EntityValidationLevelFullyCorroborated"/>
		<cmns-col:comprises rdf:resource="https://rdf.gleif.org/L1/L-UXIATLMNPCXXT5KR1S08-LEI"/>
	</owl:NamedIndividual>
	
	<owl:Class rdf:about="&fibo-fbc-fct-ireg;BusinessIdentifierCodeDataRecord">
		<rdfs:subClassOf rdf:resource="&fibo-fbc-fct-breg;BusinessRegistryEntry"/>
		<rdfs:subClassOf>
			<owl:Restriction>
				<owl:onProperty rdf:resource="&cmns-col;isIncludedIn"/>
				<owl:hasValue rdf:resource="&fibo-fbc-fct-ireg;BusinessIdentifierCodeRegistry"/>
			</owl:Restriction>
		</rdfs:subClassOf>
		<rdfs:subClassOf>
			<owl:Restriction>
				<owl:onProperty rdf:resource="&fibo-fbc-fct-breg;isSelfMaintained"/>
				<owl:someValuesFrom rdf:resource="&xsd;string"/>
			</owl:Restriction>
		</rdfs:subClassOf>
		<rdfs:subClassOf>
			<owl:Restriction>
				<owl:onProperty rdf:resource="&cmns-col;comprises"/>
				<owl:someValuesFrom rdf:resource="&fibo-fbc-fct-fse;BusinessIdentifierCode"/>
			</owl:Restriction>
		</rdfs:subClassOf>
		<rdfs:label>business identifier code data record</rdfs:label>
		<skos:definition>entry in a registry that conforms to ISO 9362 for the management of BIC codes and related registration information</skos:definition>
		<cmns-av:abbreviation>BIC data record</cmns-av:abbreviation>
		<cmns-av:adaptedFrom rdf:datatype="&xsd;anyURI">https://www.swift.com/standards/data-standards/bic</cmns-av:adaptedFrom>
	</owl:Class>
	
	<owl:NamedIndividual rdf:about="&fibo-fbc-fct-ireg;BusinessIdentifierCodeRegistrationAuthority">
		<rdf:type rdf:resource="&fibo-fbc-fct-breg;BusinessRegistrationAuthority"/>
		<rdf:type rdf:resource="&fibo-fbc-pas-fpas;FinancialServiceProvider"/>
		<rdfs:label>Business Identifier Code registration authority</rdfs:label>
		<skos:definition>registration authority and financial service provider, appointed by the International Standards Organization (ISO), that is the official registration authority (RA) for ISO 9362, Banking - Banking telecommunication messages - Business identifier code (BIC)</skos:definition>
		<fibo-fnd-rel-rel:manages rdf:resource="&fibo-fbc-fct-ireg;BusinessIdentifierCodeRegistry"/>
		<cmns-av:abbreviation>BIC RA</cmns-av:abbreviation>
		<cmns-av:abbreviation>BIC registration authority</cmns-av:abbreviation>
		<cmns-av:adaptedFrom rdf:datatype="&xsd;anyURI">https://www.swift.com/standards/data-standards/bic</cmns-av:adaptedFrom>
		<cmns-av:synonym>BIC code registrar</cmns-av:synonym>
		<cmns-rlcmp:isPlayedBy rdf:resource="&fibo-fbc-fct-ireg;SocietyForWorldwideInterbankFinancialTelecommunication"/>
	</owl:NamedIndividual>
	
	<owl:NamedIndividual rdf:about="&fibo-fbc-fct-ireg;BusinessIdentifierCodeRegistry">
		<rdf:type rdf:resource="&fibo-fbc-fct-breg;BusinessRegistry"/>
		<rdfs:label>business identifier code registry</rdfs:label>
		<skos:definition>registry for registering and maintaining information about bank and other business identifier codes that conform to ISO 9362</skos:definition>
		<fibo-fnd-rel-rel:isManagedBy rdf:resource="&fibo-fbc-fct-ireg;BusinessIdentifierCodeRegistrationAuthority"/>
		<cmns-av:abbreviation>BIC registry</cmns-av:abbreviation>
		<cmns-av:adaptedFrom rdf:datatype="&xsd;anyURI">https://www.swift.com/standards/data-standards/bic</cmns-av:adaptedFrom>
	</owl:NamedIndividual>
	
	<owl:NamedIndividual rdf:about="&fibo-fbc-fct-ireg;GLEIFLegalEntityIdentifierRegistryEntry">
		<rdf:type rdf:resource="&fibo-fbc-fct-breg;LegalEntityIdentifierRegistryEntry"/>
		<rdfs:label>Global Legal Entity Identifier Foundation (GLEIF) legal entity identifier registry entry</rdfs:label>
		<skos:definition>Global LEI Index registry entry for Global Legal Entity Identifier Foundation (GLEIF)</skos:definition>
		<fibo-fbc-fct-breg:hasInitialRegistrationDate rdf:datatype="&xsd;dateTime">2018-03-15T22:13:33-07:00</fibo-fbc-fct-breg:hasInitialRegistrationDate>
		<fibo-fbc-fct-breg:hasRegistrationRevisionDate rdf:datatype="&xsd;dateTime">2021-07-15T05:29:06-07:00</fibo-fbc-fct-breg:hasRegistrationRevisionDate>
		<fibo-fbc-fct-breg:hasRegistrationStatus rdf:resource="&fibo-fbc-fct-breg;IssuedStatus"/>
		<fibo-fbc-fct-breg:hasRenewalDate rdf:datatype="&xsd;dateTime">2022-03-15T16:00:00-07:00</fibo-fbc-fct-breg:hasRenewalDate>
		<fibo-fbc-fct-breg:hasValidationLevel rdf:resource="&fibo-fbc-fct-breg;EntityValidationLevelFullyCorroborated"/>
		<cmns-col:comprises rdf:resource="https://rdf.gleif.org/L1/L-506700GE1G29325QX363-LEI"/>
	</owl:NamedIndividual>
	
	<owl:NamedIndividual rdf:about="&fibo-fbc-fct-ireg;GlobalLEIIndex">
		<rdf:type rdf:resource="&fibo-fbc-fct-breg;LegalEntityIdentifierRegistry"/>
		<rdfs:label>Global LEI Index</rdfs:label>
		<skos:definition>registry that contains historical and current LEI records including related reference data in one authoritative, central repository</skos:definition>
		<cmns-av:explanatoryNote>The reference data provides the information on a legal entity identifiable with an LEI. The Global LEI Index is the only global online source that provides open, standardized and high quality legal entity reference data.</cmns-av:explanatoryNote>
	</owl:NamedIndividual>
	
	<owl:NamedIndividual rdf:about="&fibo-fbc-fct-ireg;GlobalLegalEntityIdentifierFoundation">
		<rdf:type rdf:resource="&fibo-be-le-fbo;NotForProfitOrganization"/>
		<rdfs:label>Global Legal Entity Identifier Foundation</rdfs:label>
		<skos:definition>Global Legal Entity Identifier Foundation (GLEIF) legal entity, tasked to support the implementation and use of the Legal Entity Identifier (LEI)</skos:definition>
		<fibo-be-le-fbo:hasHeadquartersAddress rdf:resource="&fibo-fbc-fct-ireg;GlobalLegalEntityIdentifierFoundationAddress"/>
		<fibo-be-le-lei:hasLegalAddress rdf:resource="&fibo-fbc-fct-ireg;GlobalLegalEntityIdentifierFoundationAddress"/>
		<fibo-fnd-plc-vrt:hasWebsite rdf:datatype="&xsd;anyURI">https://www.gleif.org/en/</fibo-fnd-plc-vrt:hasWebsite>
		<fibo-fnd-rel-rel:hasLegalName>Global Legal Entity Identifier Foundation</fibo-fnd-rel-rel:hasLegalName>
		<cmns-av:abbreviation>GLEIF</cmns-av:abbreviation>
	</owl:NamedIndividual>
	
	<owl:NamedIndividual rdf:about="&fibo-fbc-fct-ireg;GlobalLegalEntityIdentifierFoundationAddress">
		<rdf:type rdf:resource="&fibo-fnd-plc-adr;ConventionalStreetAddress"/>
		<rdfs:label>Global Legal Entity Identifier Foundation address</rdfs:label>
		<skos:definition>physical address of the Global Legal Entity Identifier Foundation (GLEIF)</skos:definition>
		<fibo-fnd-plc-adr:hasAddressLine1>St. Alban-Vorstadt 5</fibo-fnd-plc-adr:hasAddressLine1>
		<fibo-fnd-plc-adr:hasPostalCode>4052</fibo-fnd-plc-adr:hasPostalCode>
		<fibo-fnd-plc-loc:hasCountry rdf:resource="&lcc-3166-1;Switzerland"/>
		<fibo-fnd-plc-loc:hasMunicipality rdf:resource="&fibo-fbc-fct-bci;Basel"/>
	</owl:NamedIndividual>
	
	<owl:NamedIndividual rdf:about="&fibo-fbc-fct-ireg;IBANRegistrationAuthority">
		<rdf:type rdf:resource="&fibo-fbc-fct-ra;RegistrationAuthority"/>
		<rdf:type rdf:resource="&fibo-fbc-pas-fpas;FinancialServiceProvider"/>
		<rdfs:label>IBAN registration authority</rdfs:label>
		<skos:definition>ISO 13616:2007, International Bank Account Number (IBAN) Registration Authority (RA) and financial service provider, appointed by the International Standards Organization (ISO), that is the official registration authority (RA) for ISO 13616:2007, Financial services - International bank account number (IBAN)</skos:definition>
		<fibo-fnd-rel-rel:manages rdf:resource="&fibo-fbc-fct-ireg;BusinessIdentifierCodeRegistry"/>
		<cmns-av:adaptedFrom rdf:datatype="&xsd;anyURI">https://www.swift.com/standards/data-standards/iban</cmns-av:adaptedFrom>
		<cmns-rlcmp:isPlayedBy rdf:resource="&fibo-fbc-fct-ireg;SocietyForWorldwideInterbankFinancialTelecommunication"/>
	</owl:NamedIndividual>
	
	<owl:NamedIndividual rdf:about="&fibo-fbc-fct-ireg;LegalEntityIdentfierRegistrationAuthority">
		<rdf:type rdf:resource="&fibo-fbc-fct-ra;RegistrationAuthority"/>
		<rdfs:label>Legal Entity Identifier registration authority</rdfs:label>
		<skos:definition>registration authority appointed by the International Standards Organization (ISO) that is the official registration authority (RA) for ISO 17442, Financial services - Legal entity identifier (LEI)</skos:definition>
		<fibo-fnd-rel-rel:manages rdf:resource="&fibo-fbc-fct-ireg;GlobalLEIIndex"/>
		<cmns-rlcmp:isPlayedBy rdf:resource="&fibo-fbc-fct-ireg;GlobalLegalEntityIdentifierFoundation"/>
	</owl:NamedIndividual>
	
	<owl:NamedIndividual rdf:about="&fibo-fbc-fct-ireg;MICRegistrationAuthority">
		<rdf:type rdf:resource="&fibo-fbc-fct-ra;RegistrationAuthority"/>
		<rdf:type rdf:resource="&fibo-fbc-pas-fpas;FinancialServiceProvider"/>
		<rdfs:label>MIC registration authority</rdfs:label>
		<skos:definition>ISO 10383, Market Identifier Code (MIC) Registration Authority (RA) and financial service provider, appointed by the International Standards Organization (ISO), that is the official registration authority (RA) for ISO 10383, Codes for exchanges and market identification (MIC)</skos:definition>
		<fibo-fnd-rel-rel:manages rdf:resource="&fibo-fbc-fct-ireg;MarketIdentifierCodeRegistry"/>
		<cmns-av:abbreviation>MIC RA</cmns-av:abbreviation>
		<cmns-av:adaptedFrom rdf:datatype="&xsd;anyURI">https://www.anna-web.org/standards/mic-iso-10383/</cmns-av:adaptedFrom>
		<cmns-av:adaptedFrom rdf:datatype="&xsd;anyURI">https://www.iso20022.org/10383/iso-10383-market-identifier-codes</cmns-av:adaptedFrom>
		<cmns-av:synonym>ISO 10383 Registration Authority</cmns-av:synonym>
		<cmns-rlcmp:isPlayedBy rdf:resource="&fibo-fbc-fct-ireg;SocietyForWorldwideInterbankFinancialTelecommunication"/>
	</owl:NamedIndividual>
	
	<owl:NamedIndividual rdf:about="&fibo-fbc-fct-ireg;MarketIdentifierCodeRegistry">
		<rdf:type rdf:resource="&fibo-fbc-fct-ra;Registry"/>
		<rdfs:label>market identifier code registry</rdfs:label>
		<skos:definition>registry for registering and maintaining information for market identifier codes that conform to ISO 10383</skos:definition>
		<fibo-fnd-rel-rel:isManagedBy rdf:resource="&fibo-fbc-fct-ireg;MICRegistrationAuthority"/>
		<cmns-av:abbreviation>MIC registry</cmns-av:abbreviation>
		<cmns-av:adaptedFrom rdf:datatype="&xsd;anyURI">https://www.iso20022.org/10383/iso-10383-market-identifier-codes</cmns-av:adaptedFrom>
	</owl:NamedIndividual>
	
	<owl:Class rdf:about="&fibo-fbc-fct-ireg;MarketIdentifierCodeRegistryEntry">
		<rdfs:subClassOf rdf:resource="&fibo-fbc-fct-ra;RegistryEntry"/>
		<rdfs:subClassOf>
			<owl:Restriction>
				<owl:onProperty rdf:resource="&cmns-col;isIncludedIn"/>
				<owl:hasValue rdf:resource="&fibo-fbc-fct-ireg;MarketIdentifierCodeRegistry"/>
			</owl:Restriction>
		</rdfs:subClassOf>
		<rdfs:subClassOf>
			<owl:Restriction>
				<owl:onProperty rdf:resource="&fibo-fbc-fct-breg;hasRegistrationRevisionDate"/>
				<owl:maxQualifiedCardinality rdf:datatype="&xsd;nonNegativeInteger">1</owl:maxQualifiedCardinality>
				<owl:onDataRange rdf:resource="&xsd;string"/>
			</owl:Restriction>
		</rdfs:subClassOf>
		<rdfs:subClassOf>
			<owl:Restriction>
				<owl:onProperty rdf:resource="&fibo-fbc-fct-mkt;hasMarketIdentifierCodeStatus"/>
				<owl:onClass rdf:resource="&fibo-fbc-fct-mkt;MarketIdentifierCodeStatus"/>
				<owl:qualifiedCardinality rdf:datatype="&xsd;nonNegativeInteger">1</owl:qualifiedCardinality>
			</owl:Restriction>
		</rdfs:subClassOf>
		<rdfs:subClassOf>
			<owl:Restriction>
				<owl:onProperty rdf:resource="&fibo-fbc-fct-breg;hasInitialRegistrationDate"/>
				<owl:onDataRange rdf:resource="&xsd;string"/>
				<owl:qualifiedCardinality rdf:datatype="&xsd;nonNegativeInteger">1</owl:qualifiedCardinality>
			</owl:Restriction>
		</rdfs:subClassOf>
		<rdfs:subClassOf>
			<owl:Restriction>
				<owl:onProperty rdf:resource="&cmns-col;comprises"/>
				<owl:someValuesFrom rdf:resource="&fibo-fbc-fct-mkt;MarketIdentifier"/>
			</owl:Restriction>
		</rdfs:subClassOf>
		<rdfs:label>market identifier code registry entry</rdfs:label>
		<skos:definition>entry in a market identifier code registry that conforms to ISO 10383</skos:definition>
		<cmns-av:abbreviation>MIC registry entry</cmns-av:abbreviation>
		<cmns-av:adaptedFrom rdf:datatype="&xsd;anyURI">https://www.iso20022.org/10383/iso-10383-market-identifier-codes</cmns-av:adaptedFrom>
	</owl:Class>
	
	<owl:NamedIndividual rdf:about="&fibo-fbc-fct-ireg;SWIFTLegalEntityIdentifierRegistryEntry">
		<rdf:type rdf:resource="&fibo-fbc-fct-breg;LegalEntityIdentifierRegistryEntry"/>
		<rdfs:label>Society for Worldwide Interbank Financial Telecommunication (SWIFT) legal entity identifier registry entry</rdfs:label>
		<skos:definition>Global LEI Index registry entry for the Society for Worldwide Interbank Financial Telecommunication (SWIFT)</skos:definition>
		<fibo-fbc-fct-breg:hasInitialRegistrationDate rdf:datatype="&xsd;dateTime">2012-06-06T08:54:00-07:00</fibo-fbc-fct-breg:hasInitialRegistrationDate>
		<fibo-fbc-fct-breg:hasRegistrationRevisionDate rdf:datatype="&xsd;dateTime">2021-02-12T13:35:00-08:00</fibo-fbc-fct-breg:hasRegistrationRevisionDate>
		<fibo-fbc-fct-breg:hasRegistrationStatus rdf:resource="&fibo-fbc-fct-breg;IssuedStatus"/>
		<fibo-fbc-fct-breg:hasRenewalDate rdf:datatype="&xsd;dateTime">2022-01-20T00:21:00-08:00</fibo-fbc-fct-breg:hasRenewalDate>
		<fibo-fbc-fct-breg:hasValidationLevel rdf:resource="&fibo-fbc-fct-breg;EntityValidationLevelFullyCorroborated"/>
		<cmns-col:comprises rdf:resource="https://rdf.gleif.org/L1/L-HB7FFAZI0OMZ8PP8OE26-LEI"/>
	</owl:NamedIndividual>
	
	<owl:NamedIndividual rdf:about="&fibo-fbc-fct-ireg;SocietyForWorldwideInterbankFinancialTelecommunication">
		<rdf:type rdf:resource="&fibo-be-le-fbo;NotForProfitOrganization"/>
		<rdfs:label>Society for Worldwide Interbank Financial Telecommunication</rdfs:label>
		<skos:definition>Society for Worldwide Interbank Financial Telecommunication (SWIFT) legal entity, which is a global member-owned cooperative and the world&apos;s leading provider of secure financial messaging services</skos:definition>
		<fibo-be-le-fbo:hasHeadquartersAddress rdf:resource="&fibo-fbc-fct-ireg;SocietyForWorldwideInterbankFinancialTelecommunicationAddress"/>
		<fibo-be-le-lei:hasLegalAddress rdf:resource="&fibo-fbc-fct-ireg;SocietyForWorldwideInterbankFinancialTelecommunicationAddress"/>
		<fibo-fnd-plc-vrt:hasWebsite rdf:datatype="&xsd;anyURI">https://www.swift.com/</fibo-fnd-plc-vrt:hasWebsite>
		<fibo-fnd-rel-rel:hasLegalName>Society for Worldwide Interbank Financial Telecommunication SCRL/CVBA</fibo-fnd-rel-rel:hasLegalName>
		<cmns-av:abbreviation>SWIFT</cmns-av:abbreviation>
	</owl:NamedIndividual>
	
	<owl:NamedIndividual rdf:about="&fibo-fbc-fct-ireg;SocietyForWorldwideInterbankFinancialTelecommunicationAddress">
		<rdf:type rdf:resource="&fibo-fnd-plc-adr;ConventionalStreetAddress"/>
		<rdfs:label>Society for Worldwide Interbank Financial Telecommunication address</rdfs:label>
		<skos:definition>corporate address for the Society for Worldwide Interbank Financial Telecommunication (SWIFT)</skos:definition>
		<fibo-fnd-plc-adr:hasAddressLine1>Avenue Adèle 1</fibo-fnd-plc-adr:hasAddressLine1>
		<fibo-fnd-plc-adr:hasPostalCode>1310</fibo-fnd-plc-adr:hasPostalCode>
		<fibo-fnd-plc-loc:hasCityName>La Hulpe</fibo-fnd-plc-loc:hasCityName>
		<fibo-fnd-plc-loc:hasCountry rdf:resource="&lcc-3166-1;Belgium"/>
	</owl:NamedIndividual>

</rdf:RDF>