<?xml version="1.0" encoding="UTF-8"?>
<rdf:RDF xmlns:xsd="http://www.w3.org/2001/XMLSchema#"
         xmlns:sm="http://www.omg.org/techprocess/ab/SpecificationMetadata/"
         xmlns:fibo-fnd-utl-av="http://www.omg.org/spec/EDMC-FIBO/FND/Utilities/AnnotationVocabulary/"
         xmlns:rdf="http://www.w3.org/1999/02/22-rdf-syntax-ns#"
         xmlns:rdfs="http://www.w3.org/2000/01/rdf-schema#"
         xmlns:owl="http://www.w3.org/2002/07/owl#"
         xmlns:skos="http://www.w3.org/2004/02/skos/core#"
         xmlns:dc="http://purl.org/dc/terms/"
         xml:base="http://www.omg.org/spec/EDMC-SR/BE/FunctionalEntities/FunctionalEntities/">

   <owl:Ontology rdf:about="http://www.omg.org/spec/EDMC-SR/BE/FunctionalEntities/FunctionalEntities/">
      <owl:imports rdf:resource="http://www.omg.org/spec/EDMC-SR/BE/LegalEntities/LegalPersons/"/>
      <owl:imports rdf:resource="http://www.omg.org/spec/EDMC-SR/BE/LegalEntities/FormalBusinessOrganizations/"/>
      <owl:imports rdf:resource="http://www.edmcouncil.org/spec/EDMC-SR/FND/Relative/RelativeBusinessEntities/"/>
   </owl:Ontology>

   <!--Datatypes-->

<!--Object Properties-->

<owl:ObjectProperty rdf:about="http://www.omg.org/spec/EDMC-SR/BE/FunctionalEntities/FunctionalEntities/benefitCorporationTakesForm">
      <skos:definition>he Benefit Corporation takes the legal form of an Incorporated Company.</skos:definition>
      <rdfs:subPropertyOf rdf:resource="http://www.omg.org/spec/EDMC-SR/BE/FunctionalEntities/FunctionalEntities/functionalBusinessEntityTakesForm"/>
      <rdfs:domain rdf:resource="http://www.omg.org/spec/EDMC-SR/BE/FunctionalEntities/FunctionalEntities/BenefitCorporation"/>
      <rdfs:range rdf:resource="http://www.omg.org/spec/EDMC-SR/BE/Corporations/Corporations/IncorporatedCompany"/>
   </owl:ObjectProperty>

   <owl:ObjectProperty rdf:about="http://www.omg.org/spec/EDMC-SR/BE/FunctionalEntities/FunctionalEntities/businessIsCharacterizedBy">
      <skos:definition>A business is some entity which engages in some Commercial Activity.</skos:definition>
      <rdfs:subPropertyOf rdf:resource="http://www.omg.org/spec/EDMC-SR/BE/FunctionalEntities/FunctionalEntities/isCharacterizedBy"/>
      <rdfs:domain rdf:resource="http://www.omg.org/spec/EDMC-SR/BE/FunctionalEntities/FunctionalEntities/Business"/>
      <rdfs:range rdf:resource="http://www.omg.org/spec/EDMC-SR/BE/FunctionalEntities/FunctionalEntities/CommercialActivity"/>
   </owl:ObjectProperty>

   <owl:ObjectProperty rdf:about="http://www.omg.org/spec/EDMC-SR/BE/FunctionalEntities/FunctionalEntities/functionalBusinessEntityTakesForm">
      <skos:definition>The form which a Functional Business Entity takes. This may be any Autonomous Agent.</skos:definition>
      <rdfs:subPropertyOf rdf:resource="http://www.omg.org/spec/EDMC-SR/FND/OwnershipAndControl/Ownership/takesForm"/>
      <rdfs:subPropertyOf rdf:resource="http://www.edmcouncil.org/spec/EDMC-SR/FND/Relative/RelativeBusinessEntities/takesEntityForm"/>
      <rdfs:domain rdf:resource="http://www.omg.org/spec/EDMC-SR/BE/FunctionalEntities/FunctionalEntities/FunctionalBusinessEntity"/>
      <rdfs:range rdf:resource="http://www.omg.org/spec/EDMC-SR/FND/AgentsAndPeople/Agents/AutonomousAgent"/>
   </owl:ObjectProperty>

   <owl:ObjectProperty rdf:about="http://www.omg.org/spec/EDMC-SR/BE/FunctionalEntities/FunctionalEntities/merchantIsCharacterizedBy">
      <skos:definition>The activity for which the Merchant is set up, is commerce, that is the purchase and sale of goods.</skos:definition>
      <rdfs:subPropertyOf rdf:resource="http://www.omg.org/spec/EDMC-SR/BE/FunctionalEntities/FunctionalEntities/businessIsCharacterizedBy"/>
      <rdfs:domain rdf:resource="http://www.omg.org/spec/EDMC-SR/BE/FunctionalEntities/FunctionalEntities/Merchant"/>
      <rdfs:range rdf:resource="http://www.omg.org/spec/EDMC-SR/BE/FunctionalEntities/FunctionalEntities/Commerce"/>
   </owl:ObjectProperty>

   <owl:ObjectProperty rdf:about="http://www.omg.org/spec/EDMC-SR/BE/FunctionalEntities/FunctionalEntities/nonProfitTakesForm">
      <skos:definition>A non profit or charitable public or private foundation takes the form of a legal entity. Further Notes Per Wikipedia it is necessarily a Legal Entity. "Foundation" is this a kind of legal entity separate from the ones already defined, or another word for a kind of functional entity? Definitin Origin:Wikipedia adapted</skos:definition>
      <rdfs:subPropertyOf rdf:resource="http://www.omg.org/spec/EDMC-SR/BE/FunctionalEntities/FunctionalEntities/functionalBusinessEntityTakesForm"/>
      <rdfs:domain rdf:resource="http://www.omg.org/spec/EDMC-SR/BE/FunctionalEntities/FunctionalEntities/NonProfitOrganization"/>
      <rdfs:range rdf:resource="http://www.omg.org/spec/EDMC-SR/BE/LegalEntities/FormalBusinessOrganizations/FormallyConstitutedOrganization"/>
   </owl:ObjectProperty>

   <owl:ObjectProperty rdf:about="http://www.omg.org/spec/EDMC-SR/BE/FunctionalEntities/FunctionalEntities/soleProprietorshipTakesForm">
      <skos:definition>The person who is the proprietor or sole trader who is identified as the business.</skos:definition>
      <skos:editorialNote>Added after reviews. Captures one case where a Business Organization may have only one member, as noted at review.</skos:editorialNote>
      <rdfs:subPropertyOf rdf:resource="http://www.omg.org/spec/EDMC-SR/BE/FunctionalEntities/FunctionalEntities/functionalBusinessEntityTakesForm"/>
      <rdfs:domain rdf:resource="http://www.omg.org/spec/EDMC-SR/BE/FunctionalEntities/FunctionalEntities/SoleProprietorship"/>
      <rdfs:range rdf:resource="http://www.omg.org/spec/EDMC-SR/BE/LegalEntities/LegalPersons/NaturalPerson"/>
   </owl:ObjectProperty>

   <owl:ObjectProperty rdf:about="http://www.omg.org/spec/EDMC-SR/BE/FunctionalEntities/FunctionalEntities/isCharacterizedBy">
      <skos:definition>that context in which a contextually defined thing is defined</skos:definition>
      <rdfs:subPropertyOf rdf:resource="http://www.edmcouncil.org/spec/EDMC-SR/UO/OntologicalDegree/inContext"/>
      <rdfs:domain rdf:resource="http://www.omg.org/spec/EDMC-SR/FND/Relations/Relations/Thing"/>
      <rdfs:range rdf:resource="http://www.omg.org/spec/EDMC-SR/FND/Relations/Relations/Thing"/>
   </owl:ObjectProperty>

   <!--Data Properties-->

<!--Annotation Properties-->

<!--Classes-->

<owl:Class rdf:about="http://www.omg.org/spec/EDMC-SR/BE/FunctionalEntities/FunctionalEntities/BenefitCorporation">
      <rdfs:label>Benefit Corporation</rdfs:label>
      <skos:definition>Corporation set up under specific state legislation to provide some stated societal benefit, and with some corresponding relaxation of the obligation to maximize shareholder return.</skos:definition>
      <skos:editorialNote>This is a US-specific type of entity defined in new and emerging legislation in the US states of California, Hawaii, Virginia, Maryland, Vermont, New Jersey. Additional upcoming legislation (as at November 2011) in Colorado, New York, North Carolina, Pennsylvania, Michigan. Much of the description is framed in terms of the role of the entity rather than its nature, however the legislation specifically relaxes or otherwise changes the basic parameters of the Incorporated Company structure (for example relaxing the requirement to maximize shareholder return) It may therefore be more correct to define this as a type of Incorporated Company not a role that one sits in. Having said this, B Corporations are certified by a certifying body (B Lab), which impies that they already exist and are granted a status in a similar way to that granted to non profit enterprises. Therefore at present this is defined as a status which an Incorporated Company may attain. Web reference: www.bcorporation.net</skos:editorialNote>
      <rdfs:subClassOf rdf:resource="http://www.omg.org/spec/EDMC-SR/BE/FunctionalEntities/FunctionalEntities/FunctionalBusinessEntity"/>
   </owl:Class>

   <owl:Class rdf:about="http://www.omg.org/spec/EDMC-SR/BE/FunctionalEntities/FunctionalEntities/Business">
      <rdfs:label>Business</rdfs:label>
      <skos:definition>Some entity set up for the purposes of carrying out some commercial activities for profit.</skos:definition>
   </owl:Class>

   <owl:Class rdf:about="http://www.omg.org/spec/EDMC-SR/BE/FunctionalEntities/FunctionalEntities/Commerce">
      <rdfs:label>Commerce</rdfs:label>
      <skos:definition>The activity of buying and selling goods.</skos:definition>
      <rdfs:subClassOf rdf:resource="http://www.omg.org/spec/EDMC-SR/BE/FunctionalEntities/FunctionalEntities/CommercialActivity"/>
   </owl:Class>

   <owl:Class rdf:about="http://www.omg.org/spec/EDMC-SR/BE/FunctionalEntities/FunctionalEntities/CommercialActivity">
      <rdfs:label>Commercial Activity</rdfs:label>
      <skos:definition>The context of carrying out trade and other comercial i.e. for-profit activities.</skos:definition>
      <skos:editorialNote>This is the context which distinguishes "businesses" or commercial organizations from organizations in general, the latter including government, trans-national and non profit organizations. Note that these distinctions are usually made with reference to these kinds of context and are not necessarily reflected in the structure of those organizations.</skos:editorialNote>
      <rdfs:subClassOf rdf:resource="http://www.edmcouncil.org/spec/EDMC-SR/FND/Relative/RelativeBusinessEntities/BusinessContext"/>
   </owl:Class>

   <owl:Class rdf:about="http://www.omg.org/spec/EDMC-SR/BE/FunctionalEntities/FunctionalEntities/CooperativeSociety">
      <rdfs:label>Cooperative Society</rdfs:label>
      <skos:definition>A commercial enterprise owned and managed by and for the benefit of customers or workers.</skos:definition>
   </owl:Class>

   <owl:Class rdf:about="http://www.omg.org/spec/EDMC-SR/BE/FunctionalEntities/FunctionalEntities/FamilyOffice">
      <rdfs:label>Family Office</rdfs:label>
      <skos:definition>Family Office as defined in the relevant legislation.</skos:definition>
   </owl:Class>

   <owl:Class rdf:about="http://www.omg.org/spec/EDMC-SR/BE/FunctionalEntities/FunctionalEntities/FunctionalBusinessEntity">
      <rdfs:label>Functional Business Entity</rdfs:label>
      <skos:definition>A business entity defined in terms of its function.</skos:definition>
      <skos:editorialNote>The key distinguishing feature of a Functional Business Entity is that it may itself be constituted as some kind of Business Entity or Legal Entity, but the definition of this entity does not depend on it always having one specific legal structure (for exanple always being a limited company). This would define for example a bank, a special purpose vehicle, most government bodies and so on.</skos:editorialNote>
      <rdfs:subClassOf rdf:resource="http://www.edmcouncil.org/spec/EDMC-SR/FND/Relative/RelativeBusinessEntities/RelativeBusinessEntity"/>
   </owl:Class>

   <owl:Class rdf:about="http://www.omg.org/spec/EDMC-SR/BE/FunctionalEntities/FunctionalEntities/Merchant">
      <rdfs:label>Merchant</rdfs:label>
      <skos:definition>A business entity engaged in a trading activity. Fuether Notes: Defined in terms of its role.</skos:definition>
      <rdfs:subClassOf rdf:resource="http://www.omg.org/spec/EDMC-SR/BE/FunctionalEntities/FunctionalEntities/Business"/>
   </owl:Class>

   <owl:Class rdf:about="http://www.omg.org/spec/EDMC-SR/BE/FunctionalEntities/FunctionalEntities/NonProfitOrganization">
      <rdfs:label>Non Profit Organization</rdfs:label>
      <skos:definition>An organization which exists for some purpose other than to make a profit for its participants.</skos:definition>
      <skos:editorialNote>A non profit or charitable public or private foundation is a legal entity Action; needs a relationship to Legal Entity. Which is not a human being. Need non human legal entity scope formally defined. Probably has a board of directors.</skos:editorialNote>
   </owl:Class>

   <owl:Class rdf:about="http://www.omg.org/spec/EDMC-SR/BE/FunctionalEntities/FunctionalEntities/SoleProprietorship">
      <rdfs:label>Sole Proprietorship</rdfs:label>
      <skos:definition>A business structure in which an individual and his/her company are considered a single entity for tax and liability purposes.</skos:definition>
      <skos:editorialNote>A sole proprietorship is a company which is not registered with the state as a limited liability company or corporation. The owner does not pay income tax separately for the company, but he/she reports business income or losses on his/her individual income tax return. The owner is inseparable from the sole proprietorship, so he/she is liable for any business debts. Also called proprietorship. Definition origin:Investorwords.com</skos:editorialNote>
   </owl:Class>

   <!--Individuals-->

</rdf:RDF>