<?xml version="1.0" encoding="UTF-8"?>
  
<!DOCTYPE rdf:RDF [
    <!ENTITY fibo-fnd-plcx-gph "http://spec.edmcouncil.org/fibo/red/fnd/places-ext/geophysical/">
    <!ENTITY fibo-fnd-plc-loc "http://spec.edmcouncil.org/fibo/red/fnd/places/locations/">
    <!ENTITY fibo-fnd-plc-cty "http://spec.edmcouncil.org/fibo/red/fnd/places/countries/">
    <!ENTITY fibo-fnd-utl-bt "http://spec.edmcouncil.org/fibo/red/fnd/utilities/business-facing-types/">
]>

<rdf:RDF xmlns:xsd="http://www.w3.org/2001/XMLSchema#"
         xmlns:sm="http://www.omg.org/techprocess/ab/SpecificationMetadata/"
         xmlns:xs="http://www.w3.org/2001/XMLSchema"
         xmlns:fibo-fnd-utl-av="http://www.omg.org/spec/EDMC-FIBO/FND/Utilities/AnnotationVocabulary/"
         xmlns:rdf="http://www.w3.org/1999/02/22-rdf-syntax-ns#"
         xmlns:rdfs="http://www.w3.org/2000/01/rdf-schema#"
         xmlns:owl="http://www.w3.org/2002/07/owl#"
         xmlns:skos="http://www.w3.org/2004/02/skos/core#"
         xmlns:dc="http://purl.org/dc/terms/"
         xml:base="http://spec.edmcouncil.org/fibo/red/fnd/places-ext/geophysical/">

   <owl:Ontology rdf:about="http://spec.edmcouncil.org/fibo/red/fnd/places-ext/geophysical/">
      <owl:imports rdf:resource="http://spec.edmcouncil.org/fibo/red/fnd/places/locations/"/>
      <owl:imports rdf:resource="http://spec.edmcouncil.org/fibo/red/fnd/places/countries/"/>
      <owl:imports rdf:resource="http://spec.edmcouncil.org/fibo/red/fnd/utilities/business-facing-types/"/>
   </owl:Ontology>


  <!--
    ///////////////////////////////////////////////////////////////////////////////////////
    //
    // Datatypes
    //
    ///////////////////////////////////////////////////////////////////////////////////////
    -->



  <!--
    ///////////////////////////////////////////////////////////////////////////////////////
    //
    // Object Properties
    //
    ///////////////////////////////////////////////////////////////////////////////////////
    -->


<owl:ObjectProperty rdf:about="&fibo-fnd-plcx-gph;isLocatedIn">
      <rdfs:label>is located in</rdfs:label>
      <rdfs:domain rdf:resource="&fibo-fnd-plc-cty;UrbanCenter"/>
      <rdfs:range rdf:resource="&fibo-fnd-plc-cty;Country"/>
   </owl:ObjectProperty>


  <!--
    ///////////////////////////////////////////////////////////////////////////////////////
    //
    // Data Properties
    //
    ///////////////////////////////////////////////////////////////////////////////////////
    -->


<owl:DatatypeProperty rdf:about="&fibo-fnd-plcx-gph;name">
      <rdfs:label>name</rdfs:label>
      <skos:definition>The name of the geographical thing, as text.</skos:definition>
      <rdfs:range rdf:resource="&fibo-fnd-utl-bt;text"/>
   </owl:DatatypeProperty>


  <!--
    ///////////////////////////////////////////////////////////////////////////////////////
    //
    // Annotation Properties
    //
    ///////////////////////////////////////////////////////////////////////////////////////
    -->



  <!--
    ///////////////////////////////////////////////////////////////////////////////////////
    //
    // Classes
    //
    ///////////////////////////////////////////////////////////////////////////////////////
    -->


<owl:Class rdf:about="&fibo-fnd-plcx-gph;County">
      <rdfs:label>county</rdfs:label>
      <skos:definition>An area within a country or state, designated by that country or state as a County for its own descriptive and administrative purposes. Fiurther Notes: Specific properties of counties will vary from one country or state to another and are not erpresented here - this is purely a labelled area of land within a country, similar to a Region.</skos:definition>
      <rdfs:subClassOf rdf:resource="&fibo-fnd-plcx-gph;GeographicalArea"/>
   </owl:Class>

   <owl:Class rdf:about="&fibo-fnd-plcx-gph;GeographicalArea">
      <rdfs:label>geographical area</rdfs:label>
      <skos:definition>A named and formally defined area of the world defined in terms of its physical extent. Scope Note: A Geographical Area is both a Geographical Feature (some named physical location on Earth) and a Geophysical Location (having two-dimensional extent on the Earth's surface).</skos:definition>
      <rdfs:subClassOf rdf:resource="&fibo-fnd-plcx-gph;GeographicalFeature"/>
      <rdfs:subClassOf rdf:resource="&fibo-fnd-plcx-gph;GeophysicalLocation"/>
   </owl:Class>

   <owl:Class rdf:about="&fibo-fnd-plcx-gph;GeographicalFeature">
      <rdfs:label>geographical feature</rdfs:label>
      <skos:definition>Some named physical location on Earth, identified geographically such as a specific land area, city or geographical feature. Scope Note: This is usually an alternative way of describing some geophysical extent or location, for example describing a city as a city as distinct from describing the physical extent of that city. Many concepts may therefore extend from this and from Geophysical or Geospatial concepts. For many purposes, modelers may ignore this class. Scope Note: This differs from Geophysical Location in that may include geographical features identified as points on the Earth's surface, or as linear features such as rivers and shorelines.</skos:definition>
      <rdfs:subClassOf rdf:resource="&fibo-fnd-plc-loc;PhysicalLocation"/>
   </owl:Class>

   <owl:Class rdf:about="&fibo-fnd-plcx-gph;GeophysicalLocation">
      <rdfs:label>geophysical location</rdfs:label>
      <skos:definition>Some physical two dimensional extent on the surface of the Earth. Scope Note: The definition given in the FIBO Foundations specification for Physical Location defines some n- e.g. three dimensional space. This concept extends this to define a two dimensional extent on the Earth or other planets. Explanatory Note: Some of these locations may also be co-extensive with Geographical Features, the latter being named geophysical lications.</skos:definition>
      <rdfs:subClassOf rdf:resource="&fibo-fnd-plcx-gph;TopographicalLocation"/>
   </owl:Class>

   <owl:Class rdf:about="&fibo-fnd-plcx-gph;LandParcel">
      <rdfs:label>land parcel</rdfs:label>
      <skos:definition>Some parcel or subdivision of land.</skos:definition>
   </owl:Class>

   <owl:Class rdf:about="&fibo-fnd-plcx-gph;Neighborhood">
      <rdfs:label>neighborhood</rdfs:label>
      <skos:definition>Some residential area.</skos:definition>
   </owl:Class>

   <owl:Class rdf:about="&fibo-fnd-plcx-gph;NeighborhoodSubdivision">
      <rdfs:label>neighborhood subdivision</rdfs:label>
      <skos:definition>A block or subdivision within some residential area, commonly designated sa such for the purposes of addressing and containing within it some streets and / or residential blocks.</skos:definition>
   </owl:Class>

   <owl:Class rdf:about="&fibo-fnd-plcx-gph;Region">
      <rdfs:label>region</rdfs:label>
      <skos:definition>Some area of land, either within a country or state or encompassing several countries and states, and referred to as a Region for some purpose or other.</skos:definition>
   </owl:Class>

   <owl:Class rdf:about="&fibo-fnd-plcx-gph;Street">
      <rdfs:label>street</rdfs:label>
      <skos:definition>Some traversable strip of land or water containing along it some buildings or land.</skos:definition>
   </owl:Class>

   <owl:Class rdf:about="&fibo-fnd-plcx-gph;Territory">
      <rdfs:label>territory</rdfs:label>
      <skos:definition>A physical extent of land and water generally corresponding to the area claimed or governmed by some geopolitical entity. .</skos:definition>
   </owl:Class>

   <owl:Class rdf:about="&fibo-fnd-plcx-gph;TopographicalLocation">
      <rdfs:label>topographical location</rdfs:label>
      <skos:definition>Some physical two dimensional extent on the surface of some planet or natural satellite. Scope Note: The definition given in the FIBO Foundations specification for Physical Location defines some n- e.g. three dimensional space. This concept extends this to define a two dimensional extent on the Earth or other planets, moons etc. Scope Note: Potential specializations of this concept would include areographical locations (on Mars) and other planetographahical features. These are not in scope for FIBO but this abstraction has been included so that models which do explore that scope may be compatible with this model. Explanatory Note: Please refer to the discipline of topynymy for further details and possible extensions.</skos:definition>
   </owl:Class>


  <!--
    ///////////////////////////////////////////////////////////////////////////////////////
    //
    // Individuals
    //
    ///////////////////////////////////////////////////////////////////////////////////////
    -->


</rdf:RDF>