<?xml version="1.0" encoding="UTF-8"?>
<rdf:RDF xmlns:xsd="http://www.w3.org/2001/XMLSchema#"
         xmlns:sm="http://www.omg.org/techprocess/ab/SpecificationMetadata/"
         xmlns:fibo-fnd-utl-av="http://www.omg.org/spec/EDMC-FIBO/FND/Utilities/AnnotationVocabulary/"
         xmlns:rdf="http://www.w3.org/1999/02/22-rdf-syntax-ns#"
         xmlns:rdfs="http://www.w3.org/2000/01/rdf-schema#"
         xmlns:owl="http://www.w3.org/2002/07/owl#"
         xmlns:skos="http://www.w3.org/2004/02/skos/core#"
         xmlns:dc="http://purl.org/dc/terms/"
         xml:base="http://www.omg.org/spec/EDMC-FIBO/SEC/Securities/SecuritiesIdentification/">

   <owl:Ontology rdf:about="http://www.omg.org/spec/EDMC-FIBO/SEC/Securities/SecuritiesIdentification/">
      <owl:imports rdf:resource="http://www.omg.org/spec/EDMC-FIBO/SEC/Securities/SecuritiesIssuanceTerms/"/>
      <owl:imports rdf:resource="http://www.omg.org/spec/EDMC-FIBO/SEC/Securities/NegotiableSecurities/"/>
   </owl:Ontology>

   <!--Datatypes-->

<!--Object Properties-->

<owl:ObjectProperty rdf:about="http://www.omg.org/spec/EDMC-FIBO/SEC/Securities/SecuritiesIdentification/definedInScheme">
      <rdfs:subPropertyOf rdf:resource="http://www.omg.org/spec/EDMC-FIBO/SEC/Securities/SecuritiesIdentification/definedIn"/>
      <rdfs:domain rdf:resource="http://www.omg.org/spec/EDMC-FIBO/SEC/Securities/SecuritiesIdentification/ListedSecurityIdentifier"/>
      <rdfs:range rdf:resource="http://www.omg.org/spec/EDMC-FIBO/SEC/Securities/SecuritiesIdentification/ExchangeSecurityIdentificationScheme"/>
   </owl:ObjectProperty>

   <owl:ObjectProperty rdf:about="http://www.omg.org/spec/EDMC-FIBO/SEC/Securities/SecuritiesIdentification/hasNationalIdentifier">
      <rdfs:subPropertyOf rdf:resource="http://www.omg.org/spec/EDMC-FIBO/SEC/Securities/SecuritiesIdentification/hasSecurityIdentifier"/>
      <rdfs:domain rdf:resource="http://www.omg.org/spec/EDMC-FIBO/SEC/Securities/Securities/ExchangeTradedSecurity"/>
      <rdfs:range rdf:resource="http://www.omg.org/spec/EDMC-FIBO/SEC/Securities/SecuritiesIdentification/NationalNumberingAgencyIdentificationCode"/>
   </owl:ObjectProperty>

   <owl:ObjectProperty rdf:about="http://www.omg.org/spec/EDMC-FIBO/SEC/Securities/SecuritiesIdentification/hasIdentifier">
      <rdfs:subPropertyOf rdf:resource="http://www.omg.org/spec/EDMC-FIBO/SEC/Securities/SecuritiesIdentification/hasSecurityIdentifier"/>
      <rdfs:domain rdf:resource="http://www.omg.org/spec/EDMC-FIBO/SEC/Securities/SecuritiesIssuanceTerms/OfferIssue"/>
      <rdfs:range rdf:resource="http://www.omg.org/spec/EDMC-FIBO/SEC/Securities/SecuritiesIdentification/ListedSecurityIdentifier"/>
   </owl:ObjectProperty>

   <owl:ObjectProperty rdf:about="http://www.omg.org/spec/EDMC-FIBO/SEC/Securities/SecuritiesIdentification/canBecomePartOf">
      <skos:definition>A national identification code may become part of a more general identification code (for example, ISIN).</skos:definition>
      <rdfs:domain rdf:resource="http://www.omg.org/spec/EDMC-FIBO/SEC/Securities/SecuritiesIdentification/NationalNumberingAgencyIdentificationCode"/>
      <rdfs:range rdf:resource="http://www.omg.org/spec/EDMC-FIBO/SEC/Securities/SecuritiesIdentification/SecurityIdentifier"/>
   </owl:ObjectProperty>

   <owl:ObjectProperty rdf:about="http://www.omg.org/spec/EDMC-FIBO/SEC/Securities/SecuritiesIdentification/becomesPartOf">
      <rdfs:subPropertyOf rdf:resource="http://www.omg.org/spec/EDMC-FIBO/SEC/Securities/SecuritiesIdentification/canBecomePartOf"/>
      <rdfs:domain rdf:resource="http://www.omg.org/spec/EDMC-FIBO/SEC/Securities/SecuritiesIdentification/NationalNumberingAgencyIdentificationCode"/>
      <rdfs:range rdf:resource="http://www.omg.org/spec/EDMC-FIBO/SEC/Securities/SecuritiesIdentificationIndividuals/ISINIdentifier"/>
   </owl:ObjectProperty>

   <owl:ObjectProperty rdf:about="http://www.omg.org/spec/EDMC-FIBO/SEC/Securities/SecuritiesIdentification/definedInScheme.1">
      <rdfs:subPropertyOf rdf:resource="http://www.omg.org/spec/EDMC-FIBO/SEC/Securities/SecuritiesIdentification/definedIn"/>
      <rdfs:domain rdf:resource="http://www.omg.org/spec/EDMC-FIBO/SEC/Securities/SecuritiesIdentification/NationalNumberingAgencyIdentificationCode"/>
      <rdfs:range rdf:resource="http://www.omg.org/spec/EDMC-FIBO/SEC/Securities/SecuritiesIdentification/NationalSecurityIdentificationScheme"/>
   </owl:ObjectProperty>

   <owl:ObjectProperty rdf:about="http://www.omg.org/spec/EDMC-FIBO/SEC/Securities/SecuritiesIdentification/definedInScheme.2">
      <rdfs:subPropertyOf rdf:resource="http://www.omg.org/spec/EDMC-FIBO/SEC/Securities/SecuritiesIdentification/definedIn"/>
      <rdfs:domain rdf:resource="http://www.omg.org/spec/EDMC-FIBO/SEC/Securities/SecuritiesIdentification/ProprietarySecurityIdentificationCode"/>
      <rdfs:range rdf:resource="http://www.omg.org/spec/EDMC-FIBO/SEC/Securities/SecuritiesIdentification/ProprietarySecurityIdentificationScheme"/>
   </owl:ObjectProperty>

   <owl:ObjectProperty rdf:about="http://www.omg.org/spec/EDMC-FIBO/SEC/Securities/SecuritiesIdentification/defines">
      <rdfs:subPropertyOf rdf:resource="http://www.edmcouncil.org/spec/EDMC-SR/FND/Information/Identifiers/defines"/>
      <rdfs:domain rdf:resource="http://www.omg.org/spec/EDMC-FIBO/SEC/Securities/SecuritiesIdentification/SecurityIdentificationScheme"/>
      <rdfs:range rdf:resource="http://www.omg.org/spec/EDMC-FIBO/SEC/Securities/SecuritiesIdentification/SecurityIdentifier"/>
   </owl:ObjectProperty>

   <owl:ObjectProperty rdf:about="http://www.omg.org/spec/EDMC-FIBO/SEC/Securities/SecuritiesIdentification/definedIn">
      <rdfs:subPropertyOf rdf:resource="http://www.edmcouncil.org/spec/EDMC-SR/FND/Information/Identifiers/definedIn"/>
      <rdfs:domain rdf:resource="http://www.omg.org/spec/EDMC-FIBO/SEC/Securities/SecuritiesIdentification/SecurityIdentifier"/>
      <rdfs:range rdf:resource="http://www.omg.org/spec/EDMC-FIBO/SEC/Securities/SecuritiesIdentification/SecurityIdentificationScheme"/>
      <owl:inverseOf rdf:resource="http://www.omg.org/spec/EDMC-FIBO/SEC/Securities/SecuritiesIdentification/defines"/>
   </owl:ObjectProperty>

   <owl:ObjectProperty rdf:about="http://www.omg.org/spec/EDMC-FIBO/SEC/Securities/SecuritiesIdentification/hasSecurityIdentifier">
      <skos:definition>The primary identification code of the security. This may be any publicly defined code that is used to identify the Security.</skos:definition>
      <skos:editorialNote>Internal identifiers are out of scope of this public semantics model.</skos:editorialNote>
      <rdfs:subPropertyOf rdf:resource="http://www.edmcouncil.org/spec/EDMC-SR/FND/Information/Identifiers/hasIdentifier"/>
      <rdfs:domain rdf:resource="http://www.omg.org/spec/EDMC-FIBO/SEC/Securities/Securities/Security"/>
      <rdfs:range rdf:resource="http://www.omg.org/spec/EDMC-FIBO/SEC/Securities/SecuritiesIdentification/SecurityIdentifier"/>
   </owl:ObjectProperty>

   <!--Data Properties-->

<!--Annotation Properties-->

<!--Classes-->

<owl:Class rdf:about="http://www.omg.org/spec/EDMC-FIBO/SEC/Securities/SecuritiesIdentification/ExchangeSecurityIdentificationScheme">
      <rdfs:label>Exchange Security Identification Scheme</rdfs:label>
      <skos:definition>An identification scheme used by a securities exchange in issuing security identifiers.</skos:definition>
      <rdfs:subClassOf rdf:resource="http://www.omg.org/spec/EDMC-FIBO/SEC/Securities/SecuritiesIdentification/SecurityIdentificationScheme"/>
   </owl:Class>

   <owl:Class rdf:about="http://www.omg.org/spec/EDMC-FIBO/SEC/Securities/SecuritiesIdentification/ListedSecurityIdentifier">
      <rdfs:label>Listed Security Identifier</rdfs:label>
      <skos:definition>A Security Identifier issued in the public domain and referred to in listings etc.</skos:definition>
      <rdfs:subClassOf rdf:resource="http://www.omg.org/spec/EDMC-FIBO/SEC/Securities/SecuritiesIdentification/SecurityIdentifier"/>
   </owl:Class>

   <owl:Class rdf:about="http://www.omg.org/spec/EDMC-FIBO/SEC/Securities/SecuritiesIdentification/NationalNumberingAgencyIdentificationCode">
      <rdfs:label>National Numbering Agency Identification Code</rdfs:label>
      <skos:definition>An identifier assigned by a national numbering agency under the ISO 6166 standard.</skos:definition>
   </owl:Class>

   <owl:Class rdf:about="http://www.omg.org/spec/EDMC-FIBO/SEC/Securities/SecuritiesIdentification/NationalSecurityIdentificationScheme">
      <rdfs:label>National Security Identification Scheme</rdfs:label>
      <skos:definition>A security identification scheme published nationally on behalf of a whole country. Generally incorporated into the ISIN scheme as well.</skos:definition>
   </owl:Class>

   <owl:Class rdf:about="http://www.omg.org/spec/EDMC-FIBO/SEC/Securities/SecuritiesIdentification/ProprietarySecurityIdentificationCode">
      <rdfs:label>Proprietary Security Identification Code</rdfs:label>
      <skos:definition>An identifier supplied by a commercial data providers or governments, for example a RIC code.</skos:definition>
   </owl:Class>

   <owl:Class rdf:about="http://www.omg.org/spec/EDMC-FIBO/SEC/Securities/SecuritiesIdentification/ProprietarySecurityIdentificationScheme">
      <rdfs:label>Proprietary Security Identification Scheme</rdfs:label>
      <skos:definition>A security identification format published by a data provider or other commercial entity.</skos:definition>
   </owl:Class>

   <owl:Class rdf:about="http://www.omg.org/spec/EDMC-FIBO/SEC/Securities/SecuritiesIdentification/SecurityIdentificationScheme">
      <rdfs:label>Security Identification Scheme</rdfs:label>
      <skos:definition>A formal definition of the structure and application of a particular set of securities identifiers.</skos:definition>
      <rdfs:subClassOf rdf:resource="http://www.edmcouncil.org/spec/EDMC-SR/FND/Information/Identifiers/IdentificationScheme"/>
   </owl:Class>

   <owl:Class rdf:about="http://www.omg.org/spec/EDMC-FIBO/SEC/Securities/SecuritiesIdentification/SecurityIdentifier">
      <rdfs:label>Security Identifier</rdfs:label>
      <skos:definition>Any publicly defined code that is used to identify a Security.</skos:definition>
      <rdfs:subClassOf rdf:resource="http://www.edmcouncil.org/spec/EDMC-SR/FND/Information/Identifiers/Identifier"/>
   </owl:Class>

   <!--Individuals-->

</rdf:RDF>