<?xml version="1.0" encoding="UTF-8"?>
  
<!DOCTYPE rdf:RDF [
    <!ENTITY fibo-fnd-acc-aeq "http://spec.edmcouncil.org/fibo/red/fnd/accounting/accounting-equity/">
    <!ENTITY fibo-rl-qr "http://spec.edmcouncil.org/fibo/red/fnd/relative/quantified-resources/">
    <!ENTITY fibo-fnd-oac-own "http://spec.edmcouncil.org/fibo/red/fnd/ownership-and-control/ownership/">
    <!ENTITY fibo-be-le-fbo "http://spec.edmcouncil.org/fibo/red/be/legal-entities/formal-business-organizations/">
    <!ENTITY fibo-fnd-acc-cur "http://spec.edmcouncil.org/fibo/red/fnd/accounting/currency-amount/">
    <!ENTITY fibo-fnd-rel-rel "http://spec.edmcouncil.org/fibo/red/fnd/relations/relations/">
]>

<rdf:RDF xmlns:xsd="http://www.w3.org/2001/XMLSchema#"
         xmlns:sm="http://www.omg.org/techprocess/ab/SpecificationMetadata/"
         xmlns:xs="http://www.w3.org/2001/XMLSchema"
         xmlns:fibo-fnd-utl-av="http://www.omg.org/spec/EDMC-FIBO/FND/Utilities/AnnotationVocabulary/"
         xmlns:rdf="http://www.w3.org/1999/02/22-rdf-syntax-ns#"
         xmlns:rdfs="http://www.w3.org/2000/01/rdf-schema#"
         xmlns:owl="http://www.w3.org/2002/07/owl#"
         xmlns:skos="http://www.w3.org/2004/02/skos/core#"
         xmlns:dc="http://purl.org/dc/terms/"
         xml:base="http://spec.edmcouncil.org/fibo/red/fnd/accounting/accounting-equity/">

   <owl:Ontology rdf:about="http://spec.edmcouncil.org/fibo/red/fnd/accounting/accounting-equity/">
      <owl:imports rdf:resource="http://spec.edmcouncil.org/fibo/red/fnd/relative/quantified-resources/"/>
      <owl:imports rdf:resource="http://spec.edmcouncil.org/fibo/red/fnd/ownership-and-control/ownership/"/>
      <owl:imports rdf:resource="http://spec.edmcouncil.org/fibo/red/be/legal-entities/formal-business-organizations/"/>
      <owl:imports rdf:resource="http://spec.edmcouncil.org/fibo/red/fnd/accounting/currency-amount/"/>
      <owl:imports rdf:resource="http://spec.edmcouncil.org/fibo/red/fnd/relations/relations/"/>
   </owl:Ontology>


  <!--
    ///////////////////////////////////////////////////////////////////////////////////////
    //
    // Datatypes
    //
    ///////////////////////////////////////////////////////////////////////////////////////
    -->



  <!--
    ///////////////////////////////////////////////////////////////////////////////////////
    //
    // Object Properties
    //
    ///////////////////////////////////////////////////////////////////////////////////////
    -->


<owl:ObjectProperty rdf:about="&fibo-fnd-acc-aeq;equityRepresentsAnInterestIn">
      <rdfs:label>equity represents an interest in</rdfs:label>
      <rdfs:subPropertyOf rdf:resource="&fibo-fnd-acc-aeq;representsAnInterestIn"/>
      <rdfs:domain rdf:resource="&fibo-fnd-acc-aeq;Equity"/>
      <rdfs:range rdf:resource="&fibo-be-le-fbo;FormallyConstitutedOrganization"/>
   </owl:ObjectProperty>

   <owl:ObjectProperty rdf:about="&fibo-fnd-acc-aeq;equityTakesMaterialForm">
      <rdfs:label>equity takes material form</rdfs:label>
      <skos:definition>The amount of money represented by the Equity.</skos:definition>
      <rdfs:subPropertyOf rdf:resource="&fibo-rl-qr;quantifiedResourceTakesMaterialForm"/>
      <rdfs:subPropertyOf rdf:resource="&fibo-fnd-oac-own;takesForm"/>
      <rdfs:domain rdf:resource="&fibo-fnd-acc-aeq;Equity"/>
      <rdfs:range rdf:resource="&fibo-fnd-acc-cur;MoneyAmount"/>
   </owl:ObjectProperty>

   <owl:ObjectProperty rdf:about="&fibo-fnd-acc-aeq;hasPartCapitalSurplus">
      <rdfs:label>has part capital surplus</rdfs:label>
      <rdfs:subPropertyOf rdf:resource="&fibo-fnd-rel-rel;hasPart"/>
      <rdfs:domain rdf:resource="&fibo-fnd-acc-aeq;OwnersEquity"/>
      <rdfs:range rdf:resource="&fibo-fnd-acc-aeq;CapitalSurplus"/>
   </owl:ObjectProperty>

   <owl:ObjectProperty rdf:about="&fibo-fnd-acc-aeq;hasPartStockholdersEquity">
      <rdfs:label>has part stockholders equity</rdfs:label>
      <rdfs:subPropertyOf rdf:resource="&fibo-fnd-rel-rel;hasPart"/>
      <rdfs:domain rdf:resource="&fibo-fnd-acc-aeq;OwnersEquity"/>
      <rdfs:range rdf:resource="&fibo-fnd-acc-aeq;StockholdersEquity"/>
   </owl:ObjectProperty>

   <owl:ObjectProperty rdf:about="&fibo-fnd-acc-aeq;representsAnInterestIn">
      <rdfs:label>represents an interest in</rdfs:label>
      <skos:definition>Equity always represents an interest in some business organization. This is the organization, company or venture in which the holder of the equity has a stake in by virtue of holding that equity</skos:definition>
      <rdfs:domain rdf:resource="&fibo-fnd-rel-rel;Thing"/>
      <rdfs:range rdf:resource="&fibo-fnd-rel-rel;Thing"/>
   </owl:ObjectProperty>

   <owl:ObjectProperty rdf:about="&fibo-fnd-acc-aeq;capitalTakesMaterialForm">
      <rdfs:label>capital takes material form</rdfs:label>
      <skos:definition>The amount of money which makes up the Capital.</skos:definition>
      <rdfs:subPropertyOf rdf:resource="&fibo-fnd-oac-own;takesForm"/>
      <rdfs:subPropertyOf rdf:resource="&fibo-rl-qr;quantifiedResourceTakesMaterialForm"/>
      <rdfs:domain rdf:resource="&fibo-fnd-acc-aeq;Capital"/>
      <rdfs:range rdf:resource="&fibo-fnd-acc-cur;MoneyAmount"/>
   </owl:ObjectProperty>


  <!--
    ///////////////////////////////////////////////////////////////////////////////////////
    //
    // Data Properties
    //
    ///////////////////////////////////////////////////////////////////////////////////////
    -->



  <!--
    ///////////////////////////////////////////////////////////////////////////////////////
    //
    // Annotation Properties
    //
    ///////////////////////////////////////////////////////////////////////////////////////
    -->



  <!--
    ///////////////////////////////////////////////////////////////////////////////////////
    //
    // Classes
    //
    ///////////////////////////////////////////////////////////////////////////////////////
    -->


<owl:Class rdf:about="&fibo-fnd-acc-aeq;Equity">
      <rdfs:label>equity</rdfs:label>
      <skos:definition>the value of an ownership interest in property, including shareholders equity in a business Editorial Note: Earlier EDM Council SME Definition: "The ownership interest in some venture such as a company, a pool investment (fund) or asset pool. "</skos:definition>
   </owl:Class>

   <owl:Class rdf:about="&fibo-fnd-acc-aeq;FinancialAsset">
      <rdfs:label>financial asset</rdfs:label>
      <skos:definition>An asset consisting of one or more financial instruments, treated as an asset .</skos:definition>
      <rdfs:subClassOf rdf:resource="&fibo-fnd-oac-own;Asset"/>
   </owl:Class>

   <owl:Class rdf:about="&fibo-fnd-acc-aeq;IssuedEquity">
      <rdfs:label>issued equity</rdfs:label>
      <skos:definition>externally-held stockholders equity that may be transferred from one party to another</skos:definition>
      <rdfs:subClassOf rdf:resource="&fibo-fnd-acc-aeq;StockholdersEquity"/>
   </owl:Class>

   <owl:Class rdf:about="&fibo-fnd-acc-aeq;RetainedEarnings">
      <rdfs:label>retained earnings</rdfs:label>
      <skos:definition>In accounting, retained earnings refers to the portion of net income which is retained by the corporation rather than distributed to its owners as dividends. Similarly, if the corporation takes a loss, then that loss is retained and called variously retained losses, accumulated losses or accumulated deficit. Retained earnings and losses are cumulative from year to year with losses offsetting earnings.</skos:definition>
      <rdfs:subClassOf rdf:resource="&fibo-fnd-acc-aeq;Equity"/>
   </owl:Class>

   <owl:Class rdf:about="&fibo-fnd-acc-aeq;StockholdersEquity">
      <rdfs:label>stockholders equity</rdfs:label>
      <skos:definition>Equity held in an entity by stockholders.</skos:definition>
   </owl:Class>

   <owl:Class rdf:about="&fibo-fnd-acc-aeq;CapitalSurplus">
      <rdfs:label>capital surplus</rdfs:label>
      <skos:definition>Capital surplus is a term that frequently appears as a balance sheet item as a component of shareholders equity. Capital surplus is used to account for that amount which a firm raises in excess of the par value (nominal value) of the shares (common stock). Editorial Note: Originally labeled "additional Paid In Capital", the definition for this term is still that for Additional Paid In Capital, as sourced from Wikipedia during OMG OWL migration (2013).</skos:definition>
   </owl:Class>

   <owl:Class rdf:about="&fibo-fnd-acc-aeq;Capital">
      <rdfs:label>capital</rdfs:label>
      <skos:definition>Financial capital, which represents obligations, and is liquidated as money for trade, and owned by legal entities. It is in the form of capital assets, traded in financial markets. Its market value is not based on the historical accumulation of money invested but on the perception by the market of its expected revenues and of the risk entailed.</skos:definition>
      <rdfs:subClassOf rdf:resource="&fibo-rl-qr;QuantifiedResource"/>
   </owl:Class>

   <owl:Class rdf:about="&fibo-fnd-acc-aeq;OwnersEquity">
      <rdfs:label>owners equity</rdfs:label>
      <skos:definition>Equity owned in the entity as recorded on the books of that entity.</skos:definition>
   </owl:Class>


  <!--
    ///////////////////////////////////////////////////////////////////////////////////////
    //
    // Individuals
    //
    ///////////////////////////////////////////////////////////////////////////////////////
    -->


</rdf:RDF>