<?xml version="1.0" encoding="UTF-8"?>
<rdf:RDF xmlns:xsd="http://www.w3.org/2001/XMLSchema#"
         xmlns:sm="http://www.omg.org/techprocess/ab/SpecificationMetadata/"
         xmlns:fibo-fnd-utl-av="http://www.omg.org/spec/EDMC-FIBO/FND/Utilities/AnnotationVocabulary/"
         xmlns:rdf="http://www.w3.org/1999/02/22-rdf-syntax-ns#"
         xmlns:rdfs="http://www.w3.org/2000/01/rdf-schema#"
         xmlns:owl="http://www.w3.org/2002/07/owl#"
         xmlns:skos="http://www.w3.org/2004/02/skos/core#"
         xmlns:dc="http://purl.org/dc/terms/"
         xml:base="http://www.edmcouncil.org/spec/EDMC-SR/BE/PartnershipsExt/JurisdictionSpecificPartnerships/">

   <owl:Ontology rdf:about="http://www.edmcouncil.org/spec/EDMC-SR/BE/PartnershipsExt/JurisdictionSpecificPartnerships/">
      <owl:imports rdf:resource="http://www.omg.org/spec/EDMC-SR/BE/OwnershipAndControl/Executives/"/>
      <owl:imports rdf:resource="http://www.omg.org/spec/EDMC-SR/BE/Partnerships/Partnerships/"/>
   </owl:Ontology>

   <!--Datatypes-->

<!--Object Properties-->

<owl:ObjectProperty rdf:about="http://www.edmcouncil.org/spec/EDMC-SR/BE/PartnershipsExt/JurisdictionSpecificPartnerships/hasAgent">
      <skos:definition>The registered agent for the partnership.</skos:definition>
      <rdfs:subPropertyOf rdf:resource="http://www.omg.org/spec/EDMC-SR/BE/OwnershipAndControl/Executives/hasResponsibleParty"/>
      <rdfs:domain rdf:resource="http://www.edmcouncil.org/spec/EDMC-SR/BE/PartnershipsExt/JurisdictionSpecificPartnerships/LimitedLiabilityCompany_US_"/>
      <rdfs:range rdf:resource="http://www.edmcouncil.org/spec/EDMC-SR/BE/PartnershipsExt/JurisdictionSpecificPartnerships/LegallyIncorporatedPartershipRegisteredAgent"/>
   </owl:ObjectProperty>

   <owl:ObjectProperty rdf:about="http://www.edmcouncil.org/spec/EDMC-SR/BE/PartnershipsExt/JurisdictionSpecificPartnerships/registeredAgentIdentity">
      <skos:definition>The legal entity which is the Legally Incorporated Partnership Registered Agent</skos:definition>
      <rdfs:subPropertyOf rdf:resource="http://www.omg.org/spec/EDMC-SR/BE/OwnershipAndControl/Executives/responsiblePartyIdentity"/>
      <rdfs:domain rdf:resource="http://www.edmcouncil.org/spec/EDMC-SR/BE/PartnershipsExt/JurisdictionSpecificPartnerships/LegallyIncorporatedPartershipRegisteredAgent"/>
      <rdfs:range rdf:resource="http://www.omg.org/spec/EDMC-SR/BE/LegalEntities/LegalPersons/NaturalPerson"/>
   </owl:ObjectProperty>

   <!--Data Properties-->

<!--Annotation Properties-->

<!--Classes-->

<owl:Class rdf:about="http://www.edmcouncil.org/spec/EDMC-SR/BE/PartnershipsExt/JurisdictionSpecificPartnerships/LegallyIncorporatedPartershipRegisteredAgent">
      <rdfs:label>Legally Incorporated Partership Registered Agent</rdfs:label>
      <skos:definition>The person - usually one of the members - who will act as the entity's registered agent or agent for service of process. This is the person designated to receive legal paprts in any legal action.</skos:definition>
      <skos:editorialNote>This term is from the US LLC but is possibly applicable to other e.g. UK forms of this kind of entity.</skos:editorialNote>
      <rdfs:subClassOf rdf:resource="http://www.omg.org/spec/EDMC-SR/BE/OwnershipAndControl/Executives/ResponsibleParty"/>
   </owl:Class>

   <owl:Class rdf:about="http://www.edmcouncil.org/spec/EDMC-SR/BE/PartnershipsExt/JurisdictionSpecificPartnerships/LimitedLiabilityCompany_US_">
      <rdfs:label>Limited Liability Company (US)</rdfs:label>
      <skos:definition>A company which is a legal entity and which gives participants limited liability, but has taxation status similar to a partnership.</skos:definition>
      <skos:editorialNote>Various definitions to choose from, most of them are more descriptive than definitive. Meanwhile the UK-based ukincorp.co.uk equates a UK LLP to a US LLC. From InvestorWords: LLC. A type of company, authorized only in certain states, whose owners and managers receive the limited liability and (usually) tax benefits of an S Corporation without having to conform to the S corporation restrictions. From Money Words (ADVFN): Limited Liability Company. This is a U.S. business structure that is a cross between a partnership and a corporation. Like a corporation, the individual owners of an LLC are protected from personal liability. However, an LLC retains the partnership's benefit of having profits and losses pass to the owners without the entity itself being taxed. This business structure is ideal for small companies who are not yet ready for incorporation, but would like to avoid personal liability. From Residual Rewards: confirms this is a legal entity: LLC Definition: An LLC has characteristics of a corporation, but it is not. It does offer some of the benefits of a corporation, particularly the limitation of an owner's liability. An LLC provides lawsuit protection, credibility, tax savings, deductible employee benefits, asset protection, anonymity, the ease of raising capital, creating a separate legal entity for personal protection, an LLC has a broad range of powers beyond that of a sole proprietorship, small claims court benefits, separate liability for corporate debts, and perpetual duration. When you form an LLC you create a separate legal person and you are a shareholder. LLCs are preferred because they combine the limited liability protection of a corporation and the pass through taxation of a or partnership. The downside to an LLC is that it does not offer the free transferability of ownership, perpetual existence, and the ability to be owned by a single individual. http://www.residual-rewards.com/limited-liability-company-definition.html Definition origin:Residual Rewards Definition origin:InvestorWords.com Definition origin:advfn.com</skos:editorialNote>
      <rdfs:subClassOf rdf:resource="http://www.omg.org/spec/EDMC-SR/BE/Partnerships/Partnerships/LegallyIncorporatedPartnership"/>
   </owl:Class>

   <owl:Class rdf:about="http://www.edmcouncil.org/spec/EDMC-SR/BE/PartnershipsExt/JurisdictionSpecificPartnerships/LimitedLiabilityPartnership_UK_">
      <rdfs:label>Limited Liability Partnership (UK)</rdfs:label>
      <skos:definition>British limited liability partnership (LLP) is a new form of legal business entity with limited liability. Limited liability partnerships are taxed as partnerships but in most other respects they are very similar to companies.</skos:definition>
      <skos:editorialNote>An LLP does not have a memorandum or articles of association or a specified management structure. An LLP is also considered to be a 'Legal Person' in its own right, and can operate in the same way as a company in most respects. However, the one important difference between an LLP and a limited company is the way in which the profits are taxed, with each MEMBER of the partnership being taxed according to the share of the profits that they receive rather than the LLP paying tax directly on its profits. Detailed definition from the same source: An LLP is a body corporate and is formed by incorporation. It exists as a legal person distinct from its members. It has the legal capacity to do anything that a natural person can do. It can own UK real estate in its own right; enter into contracts; trade, develop and invest; enter into deeds; sue and be sued; enter into funding and financing agreements and grant security over its assets in its own name. It has rights, liabilities and obligations separate to and independent of its members. The liability of individual members is limited. This is to be contrasted with the liability of partners in general partnership, who are jointly and severally liable for the debts and obligations of the firm and the acts of other partners. The personal assets of a member of an LLP will not be at risk for acts of the LLP or other members. The separate legal personality of the LLP, in law, enables the liability of its members to be limited. The LLP (and not its members) will be liable to third parties.</skos:editorialNote>
   </owl:Class>

   <owl:Class rdf:about="http://www.edmcouncil.org/spec/EDMC-SR/BE/PartnershipsExt/JurisdictionSpecificPartnerships/LimitedLiabilityPartnership_US_">
      <rdfs:label>Limited Liability Partnership (US)</rdfs:label>
   </owl:Class>

   <owl:Class rdf:about="http://www.edmcouncil.org/spec/EDMC-SR/BE/PartnershipsExt/JurisdictionSpecificPartnerships/LimitedPartnership_US_">
      <rdfs:label>Limited Partnership (US)</rdfs:label>
      <skos:definition>A business organization with one or more general partners, who manage the business and assume legal debts and obligations, and one or more limited partners, who are liable only to the extent of their investments.</skos:definition>
      <skos:editorialNote>Limited partners also enjoy rights to the partnership's cash flow, but are not liable for company obligations. Provenance note: The above is US definition from InvestorWords.com for Limited Partnership. Note: Presumably this is abbreviated L.P as in Bloomberg L.P. Definition origin:InvestorWords.com</skos:editorialNote>
      <rdfs:subClassOf rdf:resource="http://www.omg.org/spec/EDMC-SR/BE/Partnerships/Partnerships/NonIncorporatedPartnership"/>
   </owl:Class>

   <!--Individuals-->

</rdf:RDF>