<?xml version="1.0" encoding="UTF-8"?>
<!DOCTYPE rdf:RDF [
	<!ENTITY dct "http://purl.org/dc/terms/">
	<!ENTITY fibo-be-oac-cown "https://spec.edmcouncil.org/fibo/ontology/BE/OwnershipAndControl/CorporateOwnership/">
	<!ENTITY fibo-be-ptr-ptr "https://spec.edmcouncil.org/fibo/ontology/BE/Partnerships/Partnerships/">
	<!ENTITY fibo-fbc-fct-fse "https://spec.edmcouncil.org/fibo/ontology/FBC/FunctionalEntities/FinancialServicesEntities/">
	<!ENTITY fibo-fbc-fi-fi "https://spec.edmcouncil.org/fibo/ontology/FBC/FinancialInstruments/FinancialInstruments/">
	<!ENTITY fibo-fbc-fi-ip "https://spec.edmcouncil.org/fibo/ontology/FBC/FinancialInstruments/InstrumentPricing/">
	<!ENTITY fibo-fbc-pas-fpas "https://spec.edmcouncil.org/fibo/ontology/FBC/ProductsAndServices/FinancialProductsAndServices/">
	<!ENTITY fibo-fnd-acc-aeq "https://spec.edmcouncil.org/fibo/ontology/FND/Accounting/AccountingEquity/">
	<!ENTITY fibo-fnd-acc-cur "https://spec.edmcouncil.org/fibo/ontology/FND/Accounting/CurrencyAmount/">
	<!ENTITY fibo-fnd-agr-agr "https://spec.edmcouncil.org/fibo/ontology/FND/Agreements/Agreements/">
	<!ENTITY fibo-fnd-agr-ctr "https://spec.edmcouncil.org/fibo/ontology/FND/Agreements/Contracts/">
	<!ENTITY fibo-fnd-arr-cls "https://spec.edmcouncil.org/fibo/ontology/FND/Arrangements/ClassificationSchemes/">
	<!ENTITY fibo-fnd-arr-lif "https://spec.edmcouncil.org/fibo/ontology/FND/Arrangements/Lifecycles/">
	<!ENTITY fibo-fnd-dt-bd "https://spec.edmcouncil.org/fibo/ontology/FND/DatesAndTimes/BusinessDates/">
	<!ENTITY fibo-fnd-dt-fd "https://spec.edmcouncil.org/fibo/ontology/FND/DatesAndTimes/FinancialDates/">
	<!ENTITY fibo-fnd-law-lcap "https://spec.edmcouncil.org/fibo/ontology/FND/Law/LegalCapacity/">
	<!ENTITY fibo-fnd-oac-own "https://spec.edmcouncil.org/fibo/ontology/FND/OwnershipAndControl/Ownership/">
	<!ENTITY fibo-fnd-pas-psch "https://spec.edmcouncil.org/fibo/ontology/FND/ProductsAndServices/PaymentsAndSchedules/">
	<!ENTITY fibo-fnd-pty-rl "https://spec.edmcouncil.org/fibo/ontology/FND/Parties/Roles/">
	<!ENTITY fibo-fnd-qt-qtu "https://spec.edmcouncil.org/fibo/ontology/FND/Quantities/QuantitiesAndUnits/">
	<!ENTITY fibo-fnd-rel-rel "https://spec.edmcouncil.org/fibo/ontology/FND/Relations/Relations/">
	<!ENTITY fibo-fnd-utl-alx "https://spec.edmcouncil.org/fibo/ontology/FND/Utilities/Analytics/">
	<!ENTITY fibo-fnd-utl-av "https://spec.edmcouncil.org/fibo/ontology/FND/Utilities/AnnotationVocabulary/">
	<!ENTITY fibo-ind-ir-ir "https://spec.edmcouncil.org/fibo/ontology/IND/InterestRates/InterestRates/">
	<!ENTITY fibo-sec-eq-eq "https://spec.edmcouncil.org/fibo/ontology/SEC/Equities/EquityInstruments/">
	<!ENTITY fibo-sec-sec-iss "https://spec.edmcouncil.org/fibo/ontology/SEC/Securities/SecuritiesIssuance/">
	<!ENTITY fibo-sec-sec-lst "https://spec.edmcouncil.org/fibo/ontology/SEC/Securities/SecuritiesListings/">
	<!ENTITY fibo-sec-sec-rst "https://spec.edmcouncil.org/fibo/ontology/SEC/Securities/SecuritiesRestrictions/">
	<!ENTITY fibo-sec-sec-sch "https://spec.edmcouncil.org/fibo/ontology/SEC/Securities/ParametricSchedules/">
	<!ENTITY lcc-cr "https://www.omg.org/spec/LCC/Countries/CountryRepresentation/">
	<!ENTITY lcc-lr "https://www.omg.org/spec/LCC/Languages/LanguageRepresentation/">
	<!ENTITY owl "http://www.w3.org/2002/07/owl#">
	<!ENTITY rdf "http://www.w3.org/1999/02/22-rdf-syntax-ns#">
	<!ENTITY rdfs "http://www.w3.org/2000/01/rdf-schema#">
	<!ENTITY skos "http://www.w3.org/2004/02/skos/core#">
	<!ENTITY sm "http://www.omg.org/techprocess/ab/SpecificationMetadata/">
	<!ENTITY xsd "http://www.w3.org/2001/XMLSchema#">
]>
<rdf:RDF xml:base="https://spec.edmcouncil.org/fibo/ontology/SEC/Equities/EquityInstruments/"
	xmlns:dct="http://purl.org/dc/terms/"
	xmlns:fibo-be-oac-cown="https://spec.edmcouncil.org/fibo/ontology/BE/OwnershipAndControl/CorporateOwnership/"
	xmlns:fibo-be-ptr-ptr="https://spec.edmcouncil.org/fibo/ontology/BE/Partnerships/Partnerships/"
	xmlns:fibo-fbc-fct-fse="https://spec.edmcouncil.org/fibo/ontology/FBC/FunctionalEntities/FinancialServicesEntities/"
	xmlns:fibo-fbc-fi-fi="https://spec.edmcouncil.org/fibo/ontology/FBC/FinancialInstruments/FinancialInstruments/"
	xmlns:fibo-fbc-fi-ip="https://spec.edmcouncil.org/fibo/ontology/FBC/FinancialInstruments/InstrumentPricing/"
	xmlns:fibo-fbc-pas-fpas="https://spec.edmcouncil.org/fibo/ontology/FBC/ProductsAndServices/FinancialProductsAndServices/"
	xmlns:fibo-fnd-acc-aeq="https://spec.edmcouncil.org/fibo/ontology/FND/Accounting/AccountingEquity/"
	xmlns:fibo-fnd-acc-cur="https://spec.edmcouncil.org/fibo/ontology/FND/Accounting/CurrencyAmount/"
	xmlns:fibo-fnd-agr-agr="https://spec.edmcouncil.org/fibo/ontology/FND/Agreements/Agreements/"
	xmlns:fibo-fnd-agr-ctr="https://spec.edmcouncil.org/fibo/ontology/FND/Agreements/Contracts/"
	xmlns:fibo-fnd-arr-cls="https://spec.edmcouncil.org/fibo/ontology/FND/Arrangements/ClassificationSchemes/"
	xmlns:fibo-fnd-arr-lif="https://spec.edmcouncil.org/fibo/ontology/FND/Arrangements/Lifecycles/"
	xmlns:fibo-fnd-dt-bd="https://spec.edmcouncil.org/fibo/ontology/FND/DatesAndTimes/BusinessDates/"
	xmlns:fibo-fnd-dt-fd="https://spec.edmcouncil.org/fibo/ontology/FND/DatesAndTimes/FinancialDates/"
	xmlns:fibo-fnd-law-lcap="https://spec.edmcouncil.org/fibo/ontology/FND/Law/LegalCapacity/"
	xmlns:fibo-fnd-oac-own="https://spec.edmcouncil.org/fibo/ontology/FND/OwnershipAndControl/Ownership/"
	xmlns:fibo-fnd-pas-psch="https://spec.edmcouncil.org/fibo/ontology/FND/ProductsAndServices/PaymentsAndSchedules/"
	xmlns:fibo-fnd-pty-rl="https://spec.edmcouncil.org/fibo/ontology/FND/Parties/Roles/"
	xmlns:fibo-fnd-qt-qtu="https://spec.edmcouncil.org/fibo/ontology/FND/Quantities/QuantitiesAndUnits/"
	xmlns:fibo-fnd-rel-rel="https://spec.edmcouncil.org/fibo/ontology/FND/Relations/Relations/"
	xmlns:fibo-fnd-utl-alx="https://spec.edmcouncil.org/fibo/ontology/FND/Utilities/Analytics/"
	xmlns:fibo-fnd-utl-av="https://spec.edmcouncil.org/fibo/ontology/FND/Utilities/AnnotationVocabulary/"
	xmlns:fibo-ind-ir-ir="https://spec.edmcouncil.org/fibo/ontology/IND/InterestRates/InterestRates/"
	xmlns:fibo-sec-eq-eq="https://spec.edmcouncil.org/fibo/ontology/SEC/Equities/EquityInstruments/"
	xmlns:fibo-sec-sec-iss="https://spec.edmcouncil.org/fibo/ontology/SEC/Securities/SecuritiesIssuance/"
	xmlns:fibo-sec-sec-lst="https://spec.edmcouncil.org/fibo/ontology/SEC/Securities/SecuritiesListings/"
	xmlns:fibo-sec-sec-rst="https://spec.edmcouncil.org/fibo/ontology/SEC/Securities/SecuritiesRestrictions/"
	xmlns:fibo-sec-sec-sch="https://spec.edmcouncil.org/fibo/ontology/SEC/Securities/ParametricSchedules/"
	xmlns:lcc-cr="https://www.omg.org/spec/LCC/Countries/CountryRepresentation/"
	xmlns:lcc-lr="https://www.omg.org/spec/LCC/Languages/LanguageRepresentation/"
	xmlns:owl="http://www.w3.org/2002/07/owl#"
	xmlns:rdf="http://www.w3.org/1999/02/22-rdf-syntax-ns#"
	xmlns:rdfs="http://www.w3.org/2000/01/rdf-schema#"
	xmlns:skos="http://www.w3.org/2004/02/skos/core#"
	xmlns:sm="http://www.omg.org/techprocess/ab/SpecificationMetadata/"
	xmlns:xsd="http://www.w3.org/2001/XMLSchema#">
	
	<owl:Ontology rdf:about="https://spec.edmcouncil.org/fibo/ontology/SEC/Equities/EquityInstruments/">
		<rdfs:label xml:lang="en">Equity Instruments Ontology</rdfs:label>
		<dct:abstract>Core terms are those fundamental to all equity instruments. This ontology also distinguishes between privately held and publicly traded equity instruments, and defines a number of related concepts, such as voting rights.</dct:abstract>
		<dct:license rdf:datatype="&xsd;anyURI">http://opensource.org/licenses/MIT</dct:license>
		<sm:contentLanguage rdf:datatype="&xsd;anyURI">http://www.w3.org/standards/techs/owl#w3c_all</sm:contentLanguage>
		<sm:copyright>Copyright (c) 2013-2020 EDM Council, Inc.</sm:copyright>
		<sm:copyright>Copyright (c) 2018-2020 Object Management Group, Inc.</sm:copyright>
		<sm:dependsOn rdf:datatype="&xsd;anyURI">https://spec.edmcouncil.org/fibo/ontology/BE/</sm:dependsOn>
		<sm:dependsOn rdf:datatype="&xsd;anyURI">https://spec.edmcouncil.org/fibo/ontology/FBC/</sm:dependsOn>
		<sm:dependsOn rdf:datatype="&xsd;anyURI">https://spec.edmcouncil.org/fibo/ontology/FND/</sm:dependsOn>
		<sm:dependsOn rdf:datatype="&xsd;anyURI">https://spec.edmcouncil.org/fibo/ontology/SEC/Securities/ParametricSchedules/</sm:dependsOn>
		<sm:dependsOn rdf:datatype="&xsd;anyURI">https://spec.edmcouncil.org/fibo/ontology/SEC/Securities/SecuritiesIssuance/</sm:dependsOn>
		<sm:dependsOn rdf:datatype="&xsd;anyURI">https://spec.edmcouncil.org/fibo/ontology/SEC/Securities/SecuritiesListings/</sm:dependsOn>
		<sm:dependsOn rdf:datatype="&xsd;anyURI">https://spec.edmcouncil.org/fibo/ontology/SEC/Securities/SecuritiesRestrictions/</sm:dependsOn>
		<sm:dependsOn rdf:datatype="&xsd;anyURI">https://www.omg.org/spec/LCC/</sm:dependsOn>
		<sm:fileAbbreviation>fibo-sec-eq-eq</sm:fileAbbreviation>
		<sm:filename>EquityInstruments.rdf</sm:filename>
		<owl:imports rdf:resource="https://spec.edmcouncil.org/fibo/ontology/BE/OwnershipAndControl/CorporateOwnership/"/>
		<owl:imports rdf:resource="https://spec.edmcouncil.org/fibo/ontology/BE/OwnershipAndControl/OwnershipParties/"/>
		<owl:imports rdf:resource="https://spec.edmcouncil.org/fibo/ontology/BE/Partnerships/Partnerships/"/>
		<owl:imports rdf:resource="https://spec.edmcouncil.org/fibo/ontology/FBC/FinancialInstruments/FinancialInstruments/"/>
		<owl:imports rdf:resource="https://spec.edmcouncil.org/fibo/ontology/FBC/FinancialInstruments/InstrumentPricing/"/>
		<owl:imports rdf:resource="https://spec.edmcouncil.org/fibo/ontology/FBC/FunctionalEntities/FinancialServicesEntities/"/>
		<owl:imports rdf:resource="https://spec.edmcouncil.org/fibo/ontology/FBC/ProductsAndServices/FinancialProductsAndServices/"/>
		<owl:imports rdf:resource="https://spec.edmcouncil.org/fibo/ontology/FND/Accounting/AccountingEquity/"/>
		<owl:imports rdf:resource="https://spec.edmcouncil.org/fibo/ontology/FND/Accounting/CurrencyAmount/"/>
		<owl:imports rdf:resource="https://spec.edmcouncil.org/fibo/ontology/FND/Agreements/Agreements/"/>
		<owl:imports rdf:resource="https://spec.edmcouncil.org/fibo/ontology/FND/Agreements/Contracts/"/>
		<owl:imports rdf:resource="https://spec.edmcouncil.org/fibo/ontology/FND/Arrangements/ClassificationSchemes/"/>
		<owl:imports rdf:resource="https://spec.edmcouncil.org/fibo/ontology/FND/Arrangements/Lifecycles/"/>
		<owl:imports rdf:resource="https://spec.edmcouncil.org/fibo/ontology/FND/DatesAndTimes/BusinessDates/"/>
		<owl:imports rdf:resource="https://spec.edmcouncil.org/fibo/ontology/FND/DatesAndTimes/FinancialDates/"/>
		<owl:imports rdf:resource="https://spec.edmcouncil.org/fibo/ontology/FND/Law/LegalCapacity/"/>
		<owl:imports rdf:resource="https://spec.edmcouncil.org/fibo/ontology/FND/OwnershipAndControl/Ownership/"/>
		<owl:imports rdf:resource="https://spec.edmcouncil.org/fibo/ontology/FND/Parties/Roles/"/>
		<owl:imports rdf:resource="https://spec.edmcouncil.org/fibo/ontology/FND/ProductsAndServices/PaymentsAndSchedules/"/>
		<owl:imports rdf:resource="https://spec.edmcouncil.org/fibo/ontology/FND/Quantities/QuantitiesAndUnits/"/>
		<owl:imports rdf:resource="https://spec.edmcouncil.org/fibo/ontology/FND/Relations/Relations/"/>
		<owl:imports rdf:resource="https://spec.edmcouncil.org/fibo/ontology/FND/Utilities/Analytics/"/>
		<owl:imports rdf:resource="https://spec.edmcouncil.org/fibo/ontology/FND/Utilities/AnnotationVocabulary/"/>
		<owl:imports rdf:resource="https://spec.edmcouncil.org/fibo/ontology/IND/InterestRates/InterestRates/"/>
		<owl:imports rdf:resource="https://spec.edmcouncil.org/fibo/ontology/SEC/Securities/ParametricSchedules/"/>
		<owl:imports rdf:resource="https://spec.edmcouncil.org/fibo/ontology/SEC/Securities/SecuritiesIssuance/"/>
		<owl:imports rdf:resource="https://spec.edmcouncil.org/fibo/ontology/SEC/Securities/SecuritiesListings/"/>
		<owl:imports rdf:resource="https://spec.edmcouncil.org/fibo/ontology/SEC/Securities/SecuritiesRestrictions/"/>
		<owl:imports rdf:resource="https://www.omg.org/spec/LCC/Countries/CountryRepresentation/"/>
		<owl:imports rdf:resource="https://www.omg.org/spec/LCC/Languages/LanguageRepresentation/"/>
		<owl:versionIRI rdf:resource="https://spec.edmcouncil.org/fibo/ontology/SEC/20201001/Equities/EquityInstruments/"/>
		<skos:changeNote>The https://spec.edmcouncil.org/fibo/ontology/SEC/20180801/Equities/EquityInstruments.rdf version of this ontology was revised to replace &apos;publicly-traded share&apos; with &apos;exchange-specific share&apos;, which is the more commonly used designation and corresponds better with the intended semantics of this concept, to merge in concepts that were formerly in a separate ShareTerms ontology, and eliminate deprecated elements.</skos:changeNote>
		<skos:changeNote>The https://spec.edmcouncil.org/fibo/ontology/SEC/20190901/Equities/EquityInstruments.rdf version of this ontology was revised to refine the definition of listed share, update definitions to remove leading articles, add missing properties and restrictions, revise the definition of dividend.</skos:changeNote>
		<skos:changeNote>The https://spec.edmcouncil.org/fibo/ontology/SEC/20191201/Equities/EquityInstruments.rdf version of this ontology was revised to refine the definition of share to include a restriction for hasSharesOutstanding, eliminate duplication of concepts in LCC, and add the concept of an equity issuer.</skos:changeNote>
		<skos:changeNote>The https://spec.edmcouncil.org/fibo/ontology/SEC/20200301/Equities/EquityInstruments.rdf version of this ontology was revised to incorporate additional features required to map the CFI classification scheme to equity instruments, including features specific to preferred shares.</skos:changeNote>
		<skos:changeNote>The https://spec.edmcouncil.org/fibo/ontology/SEC/20200801/Equities/EquityInstruments.rdf version of this ontology was revised to incorporate a property allowing representation of the share class.</skos:changeNote>
		<fibo-fnd-utl-av:hasMaturityLevel rdf:resource="&fibo-fnd-utl-av;Release"/>
	</owl:Ontology>
	
	<owl:Class rdf:about="&fibo-sec-eq-eq;AdjustableRateDividend">
		<rdfs:subClassOf rdf:resource="&fibo-sec-eq-eq;PreferredDividend"/>
		<rdfs:subClassOf>
			<owl:Restriction>
				<owl:onProperty rdf:resource="&fibo-fnd-qt-qtu;hasQuantityKind"/>
				<owl:someValuesFrom rdf:resource="&fibo-ind-ir-ir;InterestRateBenchmark"/>
			</owl:Restriction>
		</rdfs:subClassOf>
		<rdfs:subClassOf>
			<owl:Restriction>
				<owl:onProperty rdf:resource="&fibo-sec-eq-eq;hasAdjustableDividendRate"/>
				<owl:someValuesFrom rdf:resource="&fibo-fnd-acc-cur;PercentageMonetaryAmount"/>
			</owl:Restriction>
		</rdfs:subClassOf>
		<rdfs:label>adjustable rate dividend</rdfs:label>
		<skos:definition>dividend that varies with a benchmark</skos:definition>
		<fibo-fnd-utl-av:explanatoryNote>The value of the dividend from the preferred share is set by a predetermined formula to move with rates, and because of this flexibility preferred prices are often more stable then fixed-rate preferred stocks.</fibo-fnd-utl-av:explanatoryNote>
	</owl:Class>
	
	<owl:Class rdf:about="&fibo-sec-eq-eq;CommonNonVotingUnrestrictedFullyPaidRegisteredShare">
		<rdfs:subClassOf rdf:resource="&fibo-sec-eq-eq;CommonShare"/>
		<rdfs:subClassOf rdf:resource="&fibo-sec-eq-eq;UnrestrictedShare"/>
		<rdfs:subClassOf rdf:resource="&fibo-sec-sec-lst;RegisteredSecurity"/>
		<rdfs:subClassOf>
			<owl:Restriction>
				<owl:onProperty rdf:resource="&fibo-sec-eq-eq;hasSharePaymentStatus"/>
				<owl:hasValue rdf:resource="&fibo-sec-eq-eq;FullyPaidShareStatus"/>
			</owl:Restriction>
		</rdfs:subClassOf>
		<rdfs:subClassOf>
			<owl:Restriction>
				<owl:onProperty rdf:resource="&fibo-fnd-rel-rel;confers"/>
				<owl:onClass rdf:resource="&fibo-sec-eq-eq;NonVoting"/>
				<owl:qualifiedCardinality rdf:datatype="&xsd;nonNegativeInteger">1</owl:qualifiedCardinality>
			</owl:Restriction>
		</rdfs:subClassOf>
		<rdfs:subClassOf>
			<owl:Restriction>
				<owl:onProperty rdf:resource="&fibo-sec-sec-iss;isIssuedInForm"/>
				<owl:someValuesFrom rdf:resource="&fibo-sec-sec-lst;RegisteredSecurityForm"/>
			</owl:Restriction>
		</rdfs:subClassOf>
		<rdfs:label xml:lang="en-US">common, non-voting, unrestricted, fully-paid, registered share</rdfs:label>
		<skos:definition>common share that confers exactly 0 votes per share, is unrestricted from a sales perspective, is fully paid and is registered</skos:definition>
	</owl:Class>
	
	<owl:Class rdf:about="&fibo-sec-eq-eq;CommonShare">
		<rdfs:subClassOf rdf:resource="&fibo-sec-eq-eq;Share"/>
		<rdfs:subClassOf>
			<owl:Restriction>
				<owl:onProperty rdf:resource="&fibo-sec-eq-eq;pays"/>
				<owl:onClass rdf:resource="&fibo-sec-eq-eq;OrdinaryDividend"/>
				<owl:minQualifiedCardinality rdf:datatype="&xsd;nonNegativeInteger">0</owl:minQualifiedCardinality>
			</owl:Restriction>
		</rdfs:subClassOf>
		<rdfs:label xml:lang="en-US">common share</rdfs:label>
		<owl:disjointWith rdf:resource="&fibo-sec-eq-eq;PreferredShare"/>
		<skos:definition>share that signifies a unit of ownership in a corporation and represents a claim on part of the corporation&apos;s assets and earnings</skos:definition>
		<fibo-fnd-utl-av:explanatoryNote>In the event that the corporation is liquidated, claims of secured and unsecured creditors and owners of bonds and preferred shares take precedence over claims of common share holders.</fibo-fnd-utl-av:explanatoryNote>
		<fibo-fnd-utl-av:synonym xml:lang="en-GB">ordinary share</fibo-fnd-utl-av:synonym>
	</owl:Class>
	
	<owl:Class rdf:about="&fibo-sec-eq-eq;CommonVotingUnrestrictedFullyPaidRegisteredShare">
		<rdfs:subClassOf rdf:resource="&fibo-sec-eq-eq;CommonShare"/>
		<rdfs:subClassOf rdf:resource="&fibo-sec-eq-eq;UnrestrictedShare"/>
		<rdfs:subClassOf rdf:resource="&fibo-sec-sec-lst;RegisteredSecurity"/>
		<rdfs:subClassOf>
			<owl:Restriction>
				<owl:onProperty rdf:resource="&fibo-sec-eq-eq;hasSharePaymentStatus"/>
				<owl:hasValue rdf:resource="&fibo-sec-eq-eq;FullyPaidShareStatus"/>
			</owl:Restriction>
		</rdfs:subClassOf>
		<rdfs:subClassOf>
			<owl:Restriction>
				<owl:onProperty rdf:resource="&fibo-fnd-rel-rel;confers"/>
				<owl:onClass rdf:resource="&fibo-sec-eq-eq;Voting"/>
				<owl:qualifiedCardinality rdf:datatype="&xsd;nonNegativeInteger">1</owl:qualifiedCardinality>
			</owl:Restriction>
		</rdfs:subClassOf>
		<rdfs:subClassOf>
			<owl:Restriction>
				<owl:onProperty rdf:resource="&fibo-sec-sec-iss;isIssuedInForm"/>
				<owl:someValuesFrom rdf:resource="&fibo-sec-sec-lst;RegisteredSecurityForm"/>
			</owl:Restriction>
		</rdfs:subClassOf>
		<rdfs:label xml:lang="en-US">common, voting, unrestricted, fully-paid, registered share</rdfs:label>
		<skos:definition>common share that confers exactly 1 vote per share, is unrestricted from a sales perspective, is fully paid and is registered</skos:definition>
	</owl:Class>
	
	<owl:Class rdf:about="&fibo-sec-eq-eq;ConvertibleCommonShare">
		<rdfs:subClassOf rdf:resource="&fibo-sec-eq-eq;CommonShare"/>
		<rdfs:subClassOf rdf:resource="&fibo-sec-sec-iss;ConvertibleSecurity"/>
		<rdfs:label>convertible common share</rdfs:label>
		<skos:definition>common share that is convertible into another security</skos:definition>
	</owl:Class>
	
	<owl:Class rdf:about="&fibo-sec-eq-eq;ConvertiblePreferredShare">
		<rdfs:subClassOf rdf:resource="&fibo-sec-eq-eq;PreferredShare"/>
		<rdfs:subClassOf rdf:resource="&fibo-sec-sec-iss;ConvertibleSecurity"/>
		<rdfs:label>convertible preferred share</rdfs:label>
		<skos:definition>preferred share that includes an option for the holder to convert the shares into a fixed number of common shares after a predetermined date</skos:definition>
		<fibo-fnd-utl-av:explanatoryNote>Most convertible preferred stock is exchanged at the request of the shareholder, but sometimes there is a provision that allows the company, or issuer, to force conversion. The value of a convertible preferred stock is ultimately based on the performance of the common stock.</fibo-fnd-utl-av:explanatoryNote>
	</owl:Class>
	
	<owl:Class rdf:about="&fibo-sec-eq-eq;CumulativePreferredShare">
		<rdfs:subClassOf rdf:resource="&fibo-sec-eq-eq;PreferredShare"/>
		<rdfs:label>cumulative preferred share</rdfs:label>
		<skos:definition>preferred share whose dividends, if not paid due to insufficient earnings or other reasons, accumulate until paid out</skos:definition>
		<fibo-fnd-utl-av:explanatoryNote>These dividends have precedence over ordinary dividends which cannot be paid until any cumulative dividend obligations have been paid.</fibo-fnd-utl-av:explanatoryNote>
	</owl:Class>
	
	<owl:Class rdf:about="&fibo-sec-eq-eq;Custodian">
		<rdfs:subClassOf rdf:resource="&fibo-fbc-fct-fse;FinancialInstitution"/>
		<rdfs:subClassOf rdf:resource="&fibo-fbc-pas-fpas;ThirdPartyAgent"/>
		<rdfs:subClassOf>
			<owl:Restriction>
				<owl:onProperty rdf:resource="&fibo-fnd-rel-rel;holds"/>
				<owl:someValuesFrom rdf:resource="&fibo-sec-eq-eq;Share"/>
			</owl:Restriction>
		</rdfs:subClassOf>
		<rdfs:label>custodian</rdfs:label>
		<skos:definition xml:lang="en">bank or other financial institution that keeps custody of stock certificates and other assets of a mutual fund, individual, or corporate client</skos:definition>
	</owl:Class>
	
	<owl:NamedIndividual rdf:about="&fibo-sec-eq-eq;DistributionByCashPayment">
		<rdf:type rdf:resource="&fibo-sec-eq-eq;DividendDistributionMethod"/>
		<rdfs:label>distribution by payment</rdfs:label>
		<skos:definition>distribution method involving payment of cash to the shareholder</skos:definition>
	</owl:NamedIndividual>
	
	<owl:NamedIndividual rdf:about="&fibo-sec-eq-eq;DistributionByReinvestment">
		<rdf:type rdf:resource="&fibo-sec-eq-eq;DividendDistributionMethod"/>
		<rdfs:label>distribution by reinvestment</rdfs:label>
		<skos:definition>a distribution method involving automatic reinvestment of shareholders&apos; dividends in additional, potentially fractional, shares in the same equity or fund</skos:definition>
	</owl:NamedIndividual>
	
	<owl:Class rdf:about="&fibo-sec-eq-eq;Dividend">
		<rdfs:subClassOf rdf:resource="&fibo-fnd-agr-agr;Commitment"/>
		<rdfs:subClassOf>
			<owl:Restriction>
				<owl:onProperty rdf:resource="&fibo-sec-eq-eq;hasDistributionMethod"/>
				<owl:onClass rdf:resource="&fibo-sec-eq-eq;DividendDistributionMethod"/>
				<owl:maxQualifiedCardinality rdf:datatype="&xsd;nonNegativeInteger">1</owl:maxQualifiedCardinality>
			</owl:Restriction>
		</rdfs:subClassOf>
		<rdfs:subClassOf>
			<owl:Restriction>
				<owl:onProperty rdf:resource="&fibo-fnd-pas-psch;hasPaymentAmount"/>
				<owl:onClass rdf:resource="&fibo-fnd-acc-cur;MonetaryAmount"/>
				<owl:minQualifiedCardinality rdf:datatype="&xsd;nonNegativeInteger">0</owl:minQualifiedCardinality>
			</owl:Restriction>
		</rdfs:subClassOf>
		<rdfs:subClassOf>
			<owl:Restriction>
				<owl:onProperty rdf:resource="&fibo-fnd-dt-fd;hasSchedule"/>
				<owl:onClass rdf:resource="&fibo-sec-eq-eq;DividendSchedule"/>
				<owl:minQualifiedCardinality rdf:datatype="&xsd;nonNegativeInteger">0</owl:minQualifiedCardinality>
			</owl:Restriction>
		</rdfs:subClassOf>
		<rdfs:label>dividend</rdfs:label>
		<skos:definition>commitment to distribute a portion of earnings to shareholders, prorated by class of security, to be paid in the form of money, shares, scrip, or on rare occasion, property</skos:definition>
		<fibo-fnd-utl-av:explanatoryNote>The amount and timing of payment is set by the board of directors, typically quarterly.</fibo-fnd-utl-av:explanatoryNote>
	</owl:Class>
	
	<owl:Class rdf:about="&fibo-sec-eq-eq;DividendDistributionMethod">
		<rdfs:subClassOf rdf:resource="&fibo-fnd-dt-bd;Convention"/>
		<rdfs:label>dividend distribution method</rdfs:label>
		<skos:definition>convention by which dividends are distributed, i.e., by payment of a monetary amount or by reinvestment, as specified by the board of directors at the time a decision to issue a dividend is made</skos:definition>
	</owl:Class>
	
	<owl:Class rdf:about="&fibo-sec-eq-eq;DividendSchedule">
		<rdfs:subClassOf rdf:resource="&fibo-fnd-pas-psch;PaymentSchedule"/>
		<rdfs:subClassOf rdf:resource="&fibo-sec-sec-sch;ParametricSchedule"/>
		<rdfs:label>dividend schedule</rdfs:label>
		<skos:definition>payment schedule indicating the dates on which dividends are due to be paid</skos:definition>
	</owl:Class>
	
	<owl:Class rdf:about="&fibo-sec-eq-eq;EnhancedVoting">
		<rdfs:subClassOf rdf:resource="&fibo-sec-eq-eq;VotingRight"/>
		<rdfs:label>enhanced voting</rdfs:label>
		<skos:definition>shareholder is entitled to more than one vote per share</skos:definition>
	</owl:Class>
	
	<owl:Class rdf:about="&fibo-sec-eq-eq;EquityConversionTerms">
		<rdfs:subClassOf rdf:resource="&fibo-sec-sec-iss;ConversionTerms"/>
		<rdfs:subClassOf>
			<owl:Restriction>
				<owl:onProperty rdf:resource="&fibo-sec-eq-eq;specifiesConversionDate"/>
				<owl:someValuesFrom rdf:resource="&fibo-fnd-dt-fd;Date"/>
			</owl:Restriction>
		</rdfs:subClassOf>
		<rdfs:subClassOf>
			<owl:Restriction>
				<owl:onProperty rdf:resource="&fibo-sec-sec-iss;specifiesConversionInto"/>
				<owl:someValuesFrom rdf:resource="&fibo-fbc-fi-fi;Security"/>
			</owl:Restriction>
		</rdfs:subClassOf>
		<rdfs:label>equity conversion terms</rdfs:label>
		<skos:definition>conversion terms specifying the details regarding conversion of shares into other securities</skos:definition>
	</owl:Class>
	
	<owl:Class rdf:about="&fibo-sec-eq-eq;EquityIssuer">
		<rdfs:subClassOf rdf:resource="&fibo-fbc-fi-fi;Issuer"/>
		<rdfs:subClassOf>
			<owl:Restriction>
				<owl:onProperty rdf:resource="&fibo-sec-eq-eq;hasFloatingShares"/>
				<owl:minQualifiedCardinality rdf:datatype="&xsd;nonNegativeInteger">0</owl:minQualifiedCardinality>
				<owl:onDataRange rdf:resource="&xsd;nonNegativeInteger"/>
			</owl:Restriction>
		</rdfs:subClassOf>
		<rdfs:subClassOf>
			<owl:Restriction>
				<owl:onProperty rdf:resource="&fibo-sec-eq-eq;hasSharesIssued"/>
				<owl:minQualifiedCardinality rdf:datatype="&xsd;nonNegativeInteger">0</owl:minQualifiedCardinality>
				<owl:onDataRange rdf:resource="&xsd;nonNegativeInteger"/>
			</owl:Restriction>
		</rdfs:subClassOf>
		<rdfs:subClassOf>
			<owl:Restriction>
				<owl:onProperty rdf:resource="&fibo-sec-eq-eq;hasSharesOutstanding"/>
				<owl:minQualifiedCardinality rdf:datatype="&xsd;nonNegativeInteger">0</owl:minQualifiedCardinality>
				<owl:onDataRange rdf:resource="&xsd;nonNegativeInteger"/>
			</owl:Restriction>
		</rdfs:subClassOf>
		<rdfs:subClassOf>
			<owl:Restriction>
				<owl:onProperty rdf:resource="&fibo-sec-eq-eq;hasTreasuryShares"/>
				<owl:minQualifiedCardinality rdf:datatype="&xsd;nonNegativeInteger">0</owl:minQualifiedCardinality>
				<owl:onDataRange rdf:resource="&xsd;nonNegativeInteger"/>
			</owl:Restriction>
		</rdfs:subClassOf>
		<rdfs:subClassOf>
			<owl:Restriction>
				<owl:onProperty rdf:resource="&fibo-fnd-rel-rel;issues"/>
				<owl:someValuesFrom rdf:resource="&fibo-sec-eq-eq;Share"/>
			</owl:Restriction>
		</rdfs:subClassOf>
		<rdfs:label>equity issuer</rdfs:label>
		<skos:definition>issuer of shares that represent equity ownership in a corporation, or ownership in a mutual fund, or an interest in a general or limited partnership, or ownership in a structured product, such as a real estate investment trust</skos:definition>
	</owl:Class>
	
	<owl:Class rdf:about="&fibo-sec-eq-eq;EquityPosition">
		<rdfs:subClassOf rdf:resource="&fibo-fbc-pas-fpas;Position"/>
		<rdfs:subClassOf>
			<owl:Restriction>
				<owl:onProperty rdf:resource="&fibo-fnd-oac-own;hasOwningParty"/>
				<owl:onClass rdf:resource="&fibo-be-oac-cown;Shareholder"/>
				<owl:minQualifiedCardinality rdf:datatype="&xsd;nonNegativeInteger">0</owl:minQualifiedCardinality>
			</owl:Restriction>
		</rdfs:subClassOf>
		<rdfs:subClassOf>
			<owl:Restriction>
				<owl:onProperty rdf:resource="&fibo-fnd-rel-rel;isHeldBy"/>
				<owl:onClass>
					<owl:Class>
						<owl:unionOf rdf:parseType="Collection">
							<rdf:Description rdf:about="&fibo-be-oac-cown;Shareholder">
							</rdf:Description>
							<rdf:Description rdf:about="&fibo-sec-eq-eq;Custodian">
							</rdf:Description>
						</owl:unionOf>
					</owl:Class>
				</owl:onClass>
				<owl:qualifiedCardinality rdf:datatype="&xsd;nonNegativeInteger">1</owl:qualifiedCardinality>
			</owl:Restriction>
		</rdfs:subClassOf>
		<rdfs:subClassOf>
			<owl:Restriction>
				<owl:onProperty rdf:resource="&fibo-sec-eq-eq;indicatesNumberOfShares"/>
				<owl:onDataRange rdf:resource="&xsd;decimal"/>
				<owl:qualifiedCardinality rdf:datatype="&xsd;nonNegativeInteger">1</owl:qualifiedCardinality>
			</owl:Restriction>
		</rdfs:subClassOf>
		<rdfs:subClassOf>
			<owl:Restriction>
				<owl:onProperty rdf:resource="&fibo-fnd-oac-own;hasOwnedThing"/>
				<owl:someValuesFrom>
					<owl:Restriction>
						<owl:onProperty rdf:resource="&fibo-fnd-pty-rl;isPlayedBy"/>
						<owl:someValuesFrom rdf:resource="&fibo-sec-eq-eq;Share"/>
					</owl:Restriction>
				</owl:someValuesFrom>
			</owl:Restriction>
		</rdfs:subClassOf>
		<rdfs:label xml:lang="en">equity position</rdfs:label>
		<skos:definition xml:lang="en">position in an equity instrument</skos:definition>
	</owl:Class>
	
	<owl:Class rdf:about="&fibo-sec-eq-eq;EquityRedemptionProvision">
		<rdfs:subClassOf rdf:resource="&fibo-fbc-fi-fi;RedemptionProvision"/>
		<rdfs:subClassOf>
			<owl:Restriction>
				<owl:onProperty rdf:resource="&fibo-sec-eq-eq;hasMinimumRedemptionPrice"/>
				<owl:onClass rdf:resource="&fibo-fnd-acc-cur;MonetaryPrice"/>
				<owl:minQualifiedCardinality rdf:datatype="&xsd;nonNegativeInteger">0</owl:minQualifiedCardinality>
			</owl:Restriction>
		</rdfs:subClassOf>
		<rdfs:subClassOf>
			<owl:Restriction>
				<owl:onProperty rdf:resource="&fibo-sec-eq-eq;hasRedemptionPremium"/>
				<owl:onClass rdf:resource="&fibo-fnd-acc-cur;MonetaryPrice"/>
				<owl:minQualifiedCardinality rdf:datatype="&xsd;nonNegativeInteger">0</owl:minQualifiedCardinality>
			</owl:Restriction>
		</rdfs:subClassOf>
		<rdfs:subClassOf>
			<owl:Restriction>
				<owl:onProperty rdf:resource="&fibo-sec-eq-eq;hasEarliestRedemptionDate"/>
				<owl:onClass rdf:resource="&fibo-fnd-dt-fd;ExplicitDate"/>
				<owl:minQualifiedCardinality rdf:datatype="&xsd;nonNegativeInteger">0</owl:minQualifiedCardinality>
			</owl:Restriction>
		</rdfs:subClassOf>
		<rdfs:subClassOf>
			<owl:Restriction>
				<owl:onProperty rdf:resource="&fibo-sec-eq-eq;isRedeemableAtIssuerOption"/>
				<owl:minQualifiedCardinality rdf:datatype="&xsd;nonNegativeInteger">0</owl:minQualifiedCardinality>
				<owl:onDataRange rdf:resource="&xsd;boolean"/>
			</owl:Restriction>
		</rdfs:subClassOf>
		<rdfs:subClassOf>
			<owl:Restriction>
				<owl:onProperty rdf:resource="&fibo-sec-eq-eq;isRedeemableAtShareholderOption"/>
				<owl:minQualifiedCardinality rdf:datatype="&xsd;nonNegativeInteger">0</owl:minQualifiedCardinality>
				<owl:onDataRange rdf:resource="&xsd;boolean"/>
			</owl:Restriction>
		</rdfs:subClassOf>
		<rdfs:label xml:lang="en">equity redemption provision</rdfs:label>
		<skos:definition xml:lang="en">redemption provision that specifies the conditions under which the issuer or shareholder may redeem the shares</skos:definition>
	</owl:Class>
	
	<owl:Class rdf:about="&fibo-sec-eq-eq;ExtendablePreferredShare">
		<rdfs:subClassOf rdf:resource="&fibo-sec-eq-eq;RedeemablePreferredShare"/>
		<rdfs:label>extendable preferred share</rdfs:label>
		<skos:definition>redeemable preferred share whose redemption date can be extended</skos:definition>
		<skos:editorialNote>Need to add hasExtensionProvision, once that is moved from Debt</skos:editorialNote>
	</owl:Class>
	
	<owl:Class rdf:about="&fibo-sec-eq-eq;ExtraordinaryVotingRight">
		<rdfs:subClassOf rdf:resource="&fibo-sec-eq-eq;VotingRight"/>
		<rdfs:label>extraordinary voting right</rdfs:label>
		<skos:definition>right to vote at extraordinary meetings, as opposed to being able to vote strictly at annual general meetings</skos:definition>
	</owl:Class>
	
	<owl:Class rdf:about="&fibo-sec-eq-eq;FixedRateDividend">
		<rdfs:subClassOf rdf:resource="&fibo-sec-eq-eq;PreferredDividend"/>
		<rdfs:subClassOf>
			<owl:Restriction>
				<owl:onProperty rdf:resource="&fibo-sec-eq-eq;hasFixedDividendRate"/>
				<owl:someValuesFrom rdf:resource="&fibo-fnd-acc-cur;PercentageMonetaryAmount"/>
			</owl:Restriction>
		</rdfs:subClassOf>
		<rdfs:label>fixed rate dividend</rdfs:label>
		<skos:definition>dividend that provides a specified annual return on the nominal value (and any premium) paid on shares</skos:definition>
		<fibo-fnd-utl-av:explanatoryNote>In other words, the return is not variable depending on whether or not the company makes a profit.  Annual dividends are calculated as a percentage of the par value, which is the price of the preferred stock at the time it was issued. Most preferred shares have fixed rate dividends.</fibo-fnd-utl-av:explanatoryNote>
	</owl:Class>
	
	<owl:NamedIndividual rdf:about="&fibo-sec-eq-eq;FullyPaidShareStatus">
		<rdf:type rdf:resource="&fibo-sec-eq-eq;SharePaymentStatus"/>
		<rdfs:label>fully paid share status</rdfs:label>
		<skos:definition>status indicating that no additional money is owed to the company by shareholders on the value of the shares</skos:definition>
	</owl:NamedIndividual>
	
	<owl:Class rdf:about="&fibo-sec-eq-eq;LimitedPartnershipUnit">
		<rdfs:subClassOf rdf:resource="&fibo-sec-eq-eq;Share"/>
		<rdfs:subClassOf>
			<owl:Restriction>
				<owl:onProperty rdf:resource="&fibo-fnd-agr-ctr;definesTermsFor"/>
				<owl:someValuesFrom rdf:resource="&fibo-sec-eq-eq;LimitedPartnershipUnitRestriction"/>
			</owl:Restriction>
		</rdfs:subClassOf>
		<rdfs:subClassOf>
			<owl:Restriction>
				<owl:onProperty rdf:resource="&fibo-fnd-agr-ctr;hasCounterparty"/>
				<owl:someValuesFrom>
					<owl:Class>
						<owl:unionOf rdf:parseType="Collection">
							<rdf:Description rdf:about="&fibo-be-ptr-ptr;GeneralPartner">
							</rdf:Description>
							<rdf:Description rdf:about="&fibo-be-ptr-ptr;LimitedPartner">
							</rdf:Description>
						</owl:unionOf>
					</owl:Class>
				</owl:someValuesFrom>
			</owl:Restriction>
		</rdfs:subClassOf>
		<rdfs:label xml:lang="en">limited partnership unit</rdfs:label>
		<skos:definition xml:lang="en">share in a limited partnership</skos:definition>
	</owl:Class>
	
	<owl:Class rdf:about="&fibo-sec-eq-eq;LimitedPartnershipUnitRestriction">
		<rdfs:subClassOf rdf:resource="&fibo-sec-sec-rst;ContractualRestriction"/>
		<rdfs:label xml:lang="en">limited partnership unit restriction</rdfs:label>
		<skos:definition xml:lang="en">restriction on ownership or transfer of the units</skos:definition>
	</owl:Class>
	
	<owl:Class rdf:about="&fibo-sec-eq-eq;ListedShare">
		<rdfs:subClassOf rdf:resource="&fibo-sec-eq-eq;Share"/>
		<rdfs:subClassOf rdf:resource="&fibo-sec-sec-lst;ListedSecurity"/>
		<rdfs:label xml:lang="en">listed share</rdfs:label>
		<rdfs:seeAlso rdf:resource="https://www.investopedia.com/terms/l/listedsecurity.asp"/>
		<skos:definition xml:lang="en">share that is listed on one or more platforms or venues</skos:definition>
		<fibo-fnd-utl-av:explanatoryNote xml:lang="en">Listing requirements vary by exchange and include minimum stockholder&apos;s equity, a minimum share price and a minimum number of shareholders. Exchanges have listing requirements to ensure that only high quality securities are traded on them and to uphold the exchange&apos;s reputation among investors.</fibo-fnd-utl-av:explanatoryNote>
	</owl:Class>
	
	<owl:NamedIndividual rdf:about="&fibo-sec-eq-eq;NilPaidShareStatus">
		<rdf:type rdf:resource="&fibo-sec-eq-eq;SharePaymentStatus"/>
		<rdfs:label>nil paid share status</rdfs:label>
		<owl:differentFrom rdf:resource="&fibo-sec-eq-eq;FullyPaidShareStatus"/>
		<owl:differentFrom rdf:resource="&fibo-sec-eq-eq;PartiallyPaidShareStatus"/>
		<skos:definition>status indicating that none of the market value has been received by the company for the shares</skos:definition>
		<skos:example>Unpaid shares may be issued, for example, for convenience by a start-up company.</skos:example>
	</owl:NamedIndividual>
	
	<owl:Class rdf:about="&fibo-sec-eq-eq;NonCumulativePreferredShare">
		<rdfs:subClassOf rdf:resource="&fibo-sec-eq-eq;PreferredShare"/>
		<rdfs:label>non-cumulative preferred share</rdfs:label>
		<owl:disjointWith rdf:resource="&fibo-sec-eq-eq;CumulativePreferredShare"/>
		<skos:definition>preferred share whose dividend payments are not carried forward</skos:definition>
	</owl:Class>
	
	<owl:Class rdf:about="&fibo-sec-eq-eq;NonParticipatingPreferredShare">
		<rdfs:subClassOf rdf:resource="&fibo-sec-eq-eq;PreferredShare"/>
		<rdfs:label>non-participating preferred share</rdfs:label>
		<owl:disjointWith rdf:resource="&fibo-sec-eq-eq;ParticipatingPreferredShare"/>
		<skos:definition>preferred share that is not a participating preferred share</skos:definition>
	</owl:Class>
	
	<owl:Class rdf:about="&fibo-sec-eq-eq;NonVoting">
		<rdfs:subClassOf rdf:resource="&fibo-sec-eq-eq;VotingRight"/>
		<rdfs:label>non-voting</rdfs:label>
		<owl:equivalentClass>
			<owl:Restriction>
				<owl:onProperty rdf:resource="&fibo-sec-eq-eq;confersNumberOfVotesPerShare"/>
				<owl:hasValue rdf:datatype="&xsd;decimal">0</owl:hasValue>
			</owl:Restriction>
		</owl:equivalentClass>
		<skos:definition>share has no voting rights</skos:definition>
	</owl:Class>
	
	<owl:Class rdf:about="&fibo-sec-eq-eq;OrdinaryDividend">
		<rdfs:subClassOf rdf:resource="&fibo-sec-eq-eq;Dividend"/>
		<rdfs:subClassOf>
			<owl:Restriction>
				<owl:onProperty rdf:resource="&fibo-fnd-pas-psch;hasPaymentAmount"/>
				<owl:onClass rdf:resource="&fibo-fnd-acc-cur;MonetaryAmount"/>
				<owl:qualifiedCardinality rdf:datatype="&xsd;nonNegativeInteger">1</owl:qualifiedCardinality>
			</owl:Restriction>
		</rdfs:subClassOf>
		<rdfs:label>ordinary dividend</rdfs:label>
		<skos:definition>dividend that is paid to shareholders periodically</skos:definition>
		<fibo-fnd-utl-av:explanatoryNote>Most dividends are considered ordinary, unless they are specifically designated as qualified dividends.</fibo-fnd-utl-av:explanatoryNote>
		<fibo-fnd-utl-av:explanatoryNote>Note that the terms related to ordinary dividend payment are typically specified in the context of a board resolution rather than contractually.</fibo-fnd-utl-av:explanatoryNote>
	</owl:Class>
	
	<owl:Class rdf:about="&fibo-sec-eq-eq;OrdinaryVotingRight">
		<rdfs:subClassOf rdf:resource="&fibo-sec-eq-eq;VotingRight"/>
		<rdfs:label>ordinary voting right</rdfs:label>
		<skos:definition>voting right conferred on holders of common shares, as defined by the issuer</skos:definition>
	</owl:Class>
	
	<owl:NamedIndividual rdf:about="&fibo-sec-eq-eq;PartiallyPaidShareStatus">
		<rdf:type rdf:resource="&fibo-sec-eq-eq;SharePaymentStatus"/>
		<rdfs:label>partially paid share status</rdfs:label>
		<owl:differentFrom rdf:resource="&fibo-sec-eq-eq;FullyPaidShareStatus"/>
		<skos:definition>status indicating that only a portion of the market value has been received by the company for the shares</skos:definition>
		<fibo-fnd-utl-av:explanatoryNote>In the case of partially paid shares, the shareholder is still required to pay the remaining amount to the company. Typically, partially paid shares are only issued to a shareholder if there are compelling business reasons to do so.</fibo-fnd-utl-av:explanatoryNote>
	</owl:NamedIndividual>
	
	<owl:Class rdf:about="&fibo-sec-eq-eq;ParticipatingPreferredShare">
		<rdfs:subClassOf rdf:resource="&fibo-sec-eq-eq;PreferredShare"/>
		<rdfs:subClassOf>
			<owl:Restriction>
				<owl:onProperty rdf:resource="&fibo-sec-eq-eq;pays"/>
				<owl:onClass rdf:resource="&fibo-sec-eq-eq;OrdinaryDividend"/>
				<owl:minQualifiedCardinality rdf:datatype="&xsd;nonNegativeInteger">0</owl:minQualifiedCardinality>
			</owl:Restriction>
		</rdfs:subClassOf>
		<rdfs:label>participating preferred share</rdfs:label>
		<skos:definition>preferred share that, in addition to paying a stipulated dividend, gives the holder the right to participate with common share holders in additional distributions of earnings under specified conditions</skos:definition>
		<fibo-fnd-utl-av:explanatoryNote>Participating preferred shares are rare, typically only issued when needed to attract investors.</fibo-fnd-utl-av:explanatoryNote>
	</owl:Class>
	
	<owl:Class rdf:about="&fibo-sec-eq-eq;PrecedenceRight">
		<rdfs:subClassOf rdf:resource="&fibo-fnd-law-lcap;ContractualRight"/>
		<rdfs:label>precedence right</rdfs:label>
		<skos:definition>right that give the shareholder higher priority with respect to certain pre-defined dividend payments over other shareholders and that pay out first in the case of liquidation</skos:definition>
	</owl:Class>
	
	<owl:Class rdf:about="&fibo-sec-eq-eq;PreferredDividend">
		<rdfs:subClassOf rdf:resource="&fibo-sec-eq-eq;Dividend"/>
		<rdfs:subClassOf>
			<owl:Restriction>
				<owl:onProperty rdf:resource="&fibo-sec-eq-eq;hasFixedDividendRate"/>
				<owl:onClass rdf:resource="&fibo-fnd-acc-cur;PercentageMonetaryAmount"/>
				<owl:maxQualifiedCardinality rdf:datatype="&xsd;nonNegativeInteger">1</owl:maxQualifiedCardinality>
			</owl:Restriction>
		</rdfs:subClassOf>
		<rdfs:subClassOf>
			<owl:Restriction>
				<owl:onProperty rdf:resource="&fibo-sec-eq-eq;hasDividendGracePeriod"/>
				<owl:onClass rdf:resource="&fibo-fnd-dt-fd;Duration"/>
				<owl:maxQualifiedCardinality rdf:datatype="&xsd;nonNegativeInteger">1</owl:maxQualifiedCardinality>
			</owl:Restriction>
		</rdfs:subClassOf>
		<rdfs:label>preferred dividend</rdfs:label>
		<skos:definition>commitment to distribute a portion of earnings to shareholders, similar to a dividend but often with a fixed payment amount and schedule</skos:definition>
	</owl:Class>
	
	<owl:Class rdf:about="&fibo-sec-eq-eq;PreferredShare">
		<rdfs:subClassOf rdf:resource="&fibo-sec-eq-eq;Share"/>
		<rdfs:subClassOf>
			<owl:Restriction>
				<owl:onProperty rdf:resource="&fibo-fnd-rel-rel;confers"/>
				<owl:onClass rdf:resource="&fibo-sec-eq-eq;ExtraordinaryVotingRight"/>
				<owl:minQualifiedCardinality rdf:datatype="&xsd;nonNegativeInteger">0</owl:minQualifiedCardinality>
			</owl:Restriction>
		</rdfs:subClassOf>
		<rdfs:subClassOf>
			<owl:Restriction>
				<owl:onProperty rdf:resource="&fibo-sec-eq-eq;hasDividend"/>
				<owl:someValuesFrom>
					<owl:Class>
						<owl:unionOf rdf:parseType="Collection">
							<rdf:Description rdf:about="&fibo-sec-eq-eq;OrdinaryDividend">
							</rdf:Description>
							<rdf:Description rdf:about="&fibo-sec-eq-eq;PreferredDividend">
							</rdf:Description>
						</owl:unionOf>
					</owl:Class>
				</owl:someValuesFrom>
			</owl:Restriction>
		</rdfs:subClassOf>
		<rdfs:subClassOf>
			<owl:Restriction>
				<owl:onProperty rdf:resource="&fibo-sec-eq-eq;isSeniorTo"/>
				<owl:someValuesFrom rdf:resource="&fibo-sec-eq-eq;CommonShare"/>
			</owl:Restriction>
		</rdfs:subClassOf>
		<rdfs:label>preferred share</rdfs:label>
		<skos:definition>share that pays dividends at a specified rate and has preference over common shares in the payment of dividends and liquidation of corporate assets</skos:definition>
		<fibo-fnd-utl-av:synonym>preference share</fibo-fnd-utl-av:synonym>
	</owl:Class>
	
	<owl:Class rdf:about="&fibo-sec-eq-eq;PreferredShareWithAdjustableRateDividend">
		<rdfs:subClassOf rdf:resource="&fibo-sec-eq-eq;PreferredShare"/>
		<rdfs:subClassOf>
			<owl:Restriction>
				<owl:onProperty rdf:resource="&fibo-sec-eq-eq;hasDividend"/>
				<owl:someValuesFrom rdf:resource="&fibo-sec-eq-eq;AdjustableRateDividend"/>
			</owl:Restriction>
		</rdfs:subClassOf>
		<rdfs:label>preferred share with adjustable rate dividend</rdfs:label>
		<owl:disjointWith rdf:resource="&fibo-sec-eq-eq;PreferredShareWithFixedRateDividend"/>
		<skos:definition>preferred share whose dividends will vary with a benchmark, most often a T-bill rate</skos:definition>
	</owl:Class>
	
	<owl:Class rdf:about="&fibo-sec-eq-eq;PreferredShareWithFixedRateDividend">
		<rdfs:subClassOf rdf:resource="&fibo-sec-eq-eq;PreferredShare"/>
		<rdfs:subClassOf>
			<owl:Restriction>
				<owl:onProperty rdf:resource="&fibo-sec-eq-eq;hasDividend"/>
				<owl:someValuesFrom rdf:resource="&fibo-sec-eq-eq;FixedRateDividend"/>
			</owl:Restriction>
		</rdfs:subClassOf>
		<rdfs:label>preferred share with fixed rate dividend</rdfs:label>
		<skos:definition>preferred share whose dividends are set, typically according to the terms of the prospectus</skos:definition>
	</owl:Class>
	
	<owl:Class rdf:about="&fibo-sec-eq-eq;PrivatelyHeldShare">
		<rdfs:subClassOf rdf:resource="&fibo-sec-eq-eq;Share"/>
		<rdfs:label xml:lang="en">privately held share</rdfs:label>
		<owl:disjointWith rdf:resource="&fibo-sec-eq-eq;ListedShare"/>
		<skos:definition xml:lang="en">share in a security that signifies ownership in an entity that is not publicly traded</skos:definition>
		<fibo-fnd-utl-av:explanatoryNote>Privately owned companies include family-owned businesses, sole proprietorships and the vast majority of small and medium-sized businesses. These companies are often too small for an initial public offering (IPO) due, for example to a small market capitalization and/or low trading volume, and fulfill their financing requirements in other ways, including through smaller offerings.</fibo-fnd-utl-av:explanatoryNote>
	</owl:Class>
	
	<owl:Class rdf:about="&fibo-sec-eq-eq;QualifiedDividend">
		<rdfs:subClassOf rdf:resource="&fibo-sec-eq-eq;Dividend"/>
		<rdfs:label>qualified dividend</rdfs:label>
		<skos:definition>dividend that falls under capital gains tax rates that are lower than the income tax rates on unqualified, or ordinary, dividends</skos:definition>
	</owl:Class>
	
	<owl:Class rdf:about="&fibo-sec-eq-eq;RedeemablePreferredShare">
		<rdfs:subClassOf rdf:resource="&fibo-sec-eq-eq;PreferredShare"/>
		<rdfs:subClassOf>
			<owl:Restriction>
				<owl:onProperty rdf:resource="&fibo-fbc-fi-fi;hasRedemptionProvision"/>
				<owl:someValuesFrom rdf:resource="&fibo-sec-eq-eq;EquityRedemptionProvision"/>
			</owl:Restriction>
		</rdfs:subClassOf>
		<rdfs:label>redeemable preferred share</rdfs:label>
		<skos:definition>preferred share that gives the issuer (or possibly the shareholder) the right to redeem the stock under specified conditions</skos:definition>
	</owl:Class>
	
	<owl:Class rdf:about="&fibo-sec-eq-eq;RestrictedShare">
		<rdfs:subClassOf rdf:resource="&fibo-sec-eq-eq;Share"/>
		<rdfs:label xml:lang="en">restricted share</rdfs:label>
		<owl:disjointWith rdf:resource="&fibo-sec-eq-eq;UnrestrictedShare"/>
		<skos:definition xml:lang="en">share whose ownership/transfer/sale is subject to special conditions including country-specific restrictions</skos:definition>
	</owl:Class>
	
	<owl:Class rdf:about="&fibo-sec-eq-eq;RestrictedVoting">
		<rdfs:subClassOf rdf:resource="&fibo-sec-eq-eq;VotingRight"/>
		<rdfs:label>restricted voting</rdfs:label>
		<skos:definition>shareholder is restricted to less than one vote per share</skos:definition>
	</owl:Class>
	
	<owl:Class rdf:about="&fibo-sec-eq-eq;Share">
		<rdfs:subClassOf rdf:resource="&fibo-fbc-fi-fi;EquityInstrument"/>
		<rdfs:subClassOf>
			<owl:Restriction>
				<owl:onProperty rdf:resource="&fibo-sec-eq-eq;hasShareClass"/>
				<owl:minQualifiedCardinality rdf:datatype="&xsd;nonNegativeInteger">0</owl:minQualifiedCardinality>
				<owl:onDataRange rdf:resource="&xsd;string"/>
			</owl:Restriction>
		</rdfs:subClassOf>
		<rdfs:subClassOf>
			<owl:Restriction>
				<owl:onProperty rdf:resource="&fibo-fnd-rel-rel;confers"/>
				<owl:someValuesFrom rdf:resource="&fibo-sec-eq-eq;VotingRight"/>
			</owl:Restriction>
		</rdfs:subClassOf>
		<rdfs:subClassOf>
			<owl:Restriction>
				<owl:onProperty rdf:resource="&fibo-sec-eq-eq;confersOwnershipOf"/>
				<owl:someValuesFrom rdf:resource="&fibo-fnd-acc-aeq;ShareholdersEquity"/>
			</owl:Restriction>
		</rdfs:subClassOf>
		<rdfs:subClassOf>
			<owl:Restriction>
				<owl:onProperty rdf:resource="&fibo-sec-eq-eq;hasSharePaymentStatus"/>
				<owl:someValuesFrom rdf:resource="&fibo-sec-eq-eq;SharePaymentStatus"/>
			</owl:Restriction>
		</rdfs:subClassOf>
		<rdfs:label xml:lang="en">share</rdfs:label>
		<skos:definition xml:lang="en">financial instrument that signifies a unit of equity ownership in a corporation, or a unit of ownership in a mutual fund, or interest in a general or limited partnership, or a unit of ownership in a structured product, such as a real estate investment trust</skos:definition>
	</owl:Class>
	
	<owl:Class rdf:about="&fibo-sec-eq-eq;SharePaymentStatus">
		<rdfs:subClassOf rdf:resource="&fibo-fnd-arr-lif;LifecycleStatus"/>
		<rdfs:subClassOf>
			<owl:Restriction>
				<owl:onProperty rdf:resource="&lcc-cr;classifies"/>
				<owl:someValuesFrom rdf:resource="&fibo-sec-eq-eq;Share"/>
			</owl:Restriction>
		</rdfs:subClassOf>
		<rdfs:label>share payment status</rdfs:label>
		<skos:definition>classifier that specifies the overall payment status for shares issued</skos:definition>
		<fibo-fnd-utl-av:explanatoryNote>When a company issues shares upon incorporation or through an initial or secondary issuance, shareholders are required to pay a set amount for those shares. Once the company has received the full amount from shareholders, the shares become fully paid shares.</fibo-fnd-utl-av:explanatoryNote>
	</owl:Class>
	
	<owl:Class rdf:about="&fibo-sec-eq-eq;ShareYield">
		<rdfs:subClassOf rdf:resource="&fibo-fbc-fi-ip;Yield"/>
		<rdfs:subClassOf>
			<owl:Restriction>
				<owl:onProperty rdf:resource="&fibo-fnd-utl-alx;hasArgument"/>
				<owl:someValuesFrom>
					<owl:Class>
						<owl:unionOf rdf:parseType="Collection">
							<rdf:Description rdf:about="&fibo-sec-eq-eq;OrdinaryDividend">
							</rdf:Description>
							<rdf:Description rdf:about="&fibo-fbc-fi-ip;SecurityPrice">
							</rdf:Description>
						</owl:unionOf>
					</owl:Class>
				</owl:someValuesFrom>
			</owl:Restriction>
		</rdfs:subClassOf>
		<rdfs:label xml:lang="en">share yield</rdfs:label>
		<skos:definition xml:lang="en">ratio of the annualized dividend per share divided by the (current) price per share</skos:definition>
		<fibo-fnd-utl-av:synonym xml:lang="en">dividend yield</fibo-fnd-utl-av:synonym>
		<fibo-fnd-utl-av:synonym xml:lang="en">dividend-price ratio</fibo-fnd-utl-av:synonym>
	</owl:Class>
	
	<owl:Class rdf:about="&fibo-sec-eq-eq;SpecialDividend">
		<rdfs:subClassOf rdf:resource="&fibo-sec-eq-eq;Dividend"/>
		<rdfs:label>special dividend</rdfs:label>
		<skos:definition>dividend that is paid to shareholders on a one-time basis</skos:definition>
		<fibo-fnd-utl-av:usageNote xml:lang="en">Special dividends may be included in a dividend schedule as an ad-hoc entry, since they still need to be tracked based on the date of issuance.</fibo-fnd-utl-av:usageNote>
	</owl:Class>
	
	<owl:Class rdf:about="&fibo-sec-eq-eq;UnrestrictedShare">
		<rdfs:subClassOf rdf:resource="&fibo-fbc-fi-fi;NegotiableSecurity"/>
		<rdfs:subClassOf rdf:resource="&fibo-sec-eq-eq;Share"/>
		<rdfs:label xml:lang="en">unrestricted share</rdfs:label>
		<skos:definition xml:lang="en">share whose ownership/transfer/sale is not subject to special conditions including country-specific restrictions</skos:definition>
	</owl:Class>
	
	<owl:Class rdf:about="&fibo-sec-eq-eq;Voting">
		<rdfs:subClassOf rdf:resource="&fibo-sec-eq-eq;VotingRight"/>
		<rdfs:label>voting</rdfs:label>
		<owl:equivalentClass>
			<owl:Restriction>
				<owl:onProperty rdf:resource="&fibo-sec-eq-eq;confersNumberOfVotesPerShare"/>
				<owl:hasValue rdf:datatype="&xsd;decimal">1</owl:hasValue>
			</owl:Restriction>
		</owl:equivalentClass>
		<skos:definition>right that confers exactly one vote per share</skos:definition>
	</owl:Class>
	
	<owl:Class rdf:about="&fibo-sec-eq-eq;VotingRight">
		<rdfs:subClassOf rdf:resource="&fibo-fnd-law-lcap;ContractualRight"/>
		<rdfs:subClassOf>
			<owl:Restriction>
				<owl:onProperty rdf:resource="&fibo-sec-eq-eq;hasVotingRestriction"/>
				<owl:minQualifiedCardinality rdf:datatype="&xsd;nonNegativeInteger">0</owl:minQualifiedCardinality>
				<owl:onDataRange rdf:resource="&xsd;string"/>
			</owl:Restriction>
		</rdfs:subClassOf>
		<rdfs:subClassOf>
			<owl:Restriction>
				<owl:onProperty rdf:resource="&fibo-sec-eq-eq;confersNumberOfVotesPerShare"/>
				<owl:onDataRange rdf:resource="&xsd;decimal"/>
				<owl:qualifiedCardinality rdf:datatype="&xsd;nonNegativeInteger">1</owl:qualifiedCardinality>
			</owl:Restriction>
		</rdfs:subClassOf>
		<rdfs:subClassOf>
			<owl:Restriction>
				<owl:onProperty rdf:resource="&fibo-fnd-rel-rel;isConferredBy"/>
				<owl:someValuesFrom rdf:resource="&fibo-fnd-agr-ctr;WrittenContract"/>
			</owl:Restriction>
		</rdfs:subClassOf>
		<rdfs:label>voting right</rdfs:label>
		<skos:definition>contractual right that specifies shareholder voting entitlements, such as to elect directors, elect outside auditors, and vote on matters of corporate policy</skos:definition>
		<fibo-fnd-utl-av:explanatoryNote>Voting may involve decisions on issuing securities, initiating stock splits, and making substantial changes in the corporation&apos;s operations.  Note that a given share may not have voting rights, in which case the number of votes per share would be zero.</fibo-fnd-utl-av:explanatoryNote>
	</owl:Class>
	
	<owl:DatatypeProperty rdf:about="&fibo-sec-eq-eq;confersNumberOfVotesPerShare">
		<rdfs:subPropertyOf rdf:resource="&fibo-fnd-acc-cur;hasAmount"/>
		<rdfs:label xml:lang="en">number of votes per share</rdfs:label>
		<rdfs:domain rdf:resource="&fibo-sec-eq-eq;VotingRight"/>
		<rdfs:range rdf:resource="&xsd;decimal"/>
		<skos:definition xml:lang="en">grants the right to vote on a per share basis to the shareholder</skos:definition>
		<fibo-fnd-utl-av:explanatoryNote xml:lang="en">Voting rights may be set at zero, one, or more votes per share, depending on the contract.</fibo-fnd-utl-av:explanatoryNote>
	</owl:DatatypeProperty>
	
	<owl:ObjectProperty rdf:about="&fibo-sec-eq-eq;confersOwnershipOf">
		<rdfs:subPropertyOf rdf:resource="&fibo-fnd-rel-rel;confers"/>
		<rdfs:label>confers ownership of</rdfs:label>
		<rdfs:domain rdf:resource="&fibo-fnd-agr-ctr;Contract"/>
		<skos:definition xml:lang="en">grants or bestows ownership via contract</skos:definition>
	</owl:ObjectProperty>
	
	<owl:ObjectProperty rdf:about="&fibo-sec-eq-eq;hasAdjustableDividendRate">
		<rdfs:subPropertyOf rdf:resource="&lcc-lr;has"/>
		<rdfs:label>has adjustable dividend rate</rdfs:label>
		<rdfs:domain rdf:resource="&fibo-sec-eq-eq;PreferredDividend"/>
		<rdfs:range rdf:resource="&fibo-fnd-acc-cur;PercentageMonetaryAmount"/>
		<skos:definition>indicates the pre-arranged variable dividend rate, typically specified in the prospectus as a formula based on a benchmark, for a preferred share</skos:definition>
	</owl:ObjectProperty>
	
	<owl:ObjectProperty rdf:about="&fibo-sec-eq-eq;hasDistributionMethod">
		<rdfs:subPropertyOf rdf:resource="&lcc-lr;has"/>
		<rdfs:label>has distribution method</rdfs:label>
		<rdfs:domain rdf:resource="&fibo-sec-eq-eq;Dividend"/>
		<rdfs:range rdf:resource="&fibo-sec-eq-eq;DividendDistributionMethod"/>
		<skos:definition>indicates the method by which dividend payments are to be distributed</skos:definition>
	</owl:ObjectProperty>
	
	<owl:ObjectProperty rdf:about="&fibo-sec-eq-eq;hasDividend">
		<rdfs:subPropertyOf rdf:resource="&lcc-lr;has"/>
		<rdfs:label>has dividend</rdfs:label>
		<rdfs:domain rdf:resource="&fibo-sec-eq-eq;Share"/>
		<rdfs:range>
			<owl:Class>
				<owl:unionOf rdf:parseType="Collection">
					<rdf:Description rdf:about="&fibo-sec-eq-eq;OrdinaryDividend">
					</rdf:Description>
					<rdf:Description rdf:about="&fibo-sec-eq-eq;PreferredDividend">
					</rdf:Description>
				</owl:unionOf>
			</owl:Class>
		</rdfs:range>
		<skos:definition>relates a share to a dividend that applies to that share</skos:definition>
	</owl:ObjectProperty>
	
	<owl:ObjectProperty rdf:about="&fibo-sec-eq-eq;hasDividendDeclarationDate">
		<rdfs:subPropertyOf rdf:resource="&fibo-fnd-dt-fd;hasExplicitDate"/>
		<rdfs:label>has declaration date</rdfs:label>
		<rdfs:domain rdf:resource="&fibo-sec-eq-eq;Share"/>
		<rdfs:range rdf:resource="&fibo-fnd-dt-fd;ExplicitDate"/>
		<skos:definition>indicates a date on which an organization states that a dividend payment may be anticipated, including the the dividend amount and the ex-dividend and payment dates</skos:definition>
		<fibo-fnd-utl-av:synonym>has announcement date</fibo-fnd-utl-av:synonym>
	</owl:ObjectProperty>
	
	<owl:ObjectProperty rdf:about="&fibo-sec-eq-eq;hasDividendGracePeriod">
		<rdfs:subPropertyOf rdf:resource="&fibo-fnd-dt-fd;hasDuration"/>
		<rdfs:label>has dividend grace period</rdfs:label>
		<rdfs:domain rdf:resource="&fibo-sec-eq-eq;PreferredDividend"/>
		<rdfs:range rdf:resource="&fibo-fnd-dt-fd;Duration"/>
		<skos:definition>indicates a period of time after a dividend payment becomes due, before the issuer is subject to penalties</skos:definition>
	</owl:ObjectProperty>
	
	<owl:ObjectProperty rdf:about="&fibo-sec-eq-eq;hasEarliestRedemptionDate">
		<rdfs:subPropertyOf rdf:resource="&fibo-fnd-dt-fd;hasExplicitDate"/>
		<rdfs:label>has earliest redemption date</rdfs:label>
		<rdfs:domain rdf:resource="&fibo-sec-eq-eq;EquityRedemptionProvision"/>
		<rdfs:range rdf:resource="&fibo-fnd-dt-fd;ExplicitDate"/>
		<skos:definition>indicates a date on or after which a stock can be redeemed</skos:definition>
	</owl:ObjectProperty>
	
	<owl:ObjectProperty rdf:about="&fibo-sec-eq-eq;hasExDividendDate">
		<rdfs:subPropertyOf rdf:resource="&fibo-fnd-dt-fd;hasExplicitDate"/>
		<rdfs:label>has ex-dividend date</rdfs:label>
		<rdfs:domain rdf:resource="&fibo-sec-eq-eq;Share"/>
		<rdfs:range rdf:resource="&fibo-fnd-dt-fd;ExplicitDate"/>
		<skos:definition>indicates a date on which a stock &apos;goes ex-dividend&apos;, typically about three weeks before the dividend is paid to shareholders of record</skos:definition>
		<fibo-fnd-utl-av:adaptedFrom rdf:datatype="&xsd;anyURI">https://www.investor.gov/introduction-investing/investing-basics/glossary/ex-dividend-dates-when-are-you-entitled-stock-and</fibo-fnd-utl-av:adaptedFrom>
		<fibo-fnd-utl-av:explanatoryNote>Once the company sets the record date, the ex-dividend date is set based on stock exchange rules. If you purchase a stock on its ex-dividend date or after, you will not receive the next dividend payment.</fibo-fnd-utl-av:explanatoryNote>
		<fibo-fnd-utl-av:explanatoryNote>Shares listed on the New York Stock Exchange go ex-dividend four business days prior to the record date.</fibo-fnd-utl-av:explanatoryNote>
		<fibo-fnd-utl-av:synonym>has ex-date</fibo-fnd-utl-av:synonym>
		<fibo-fnd-utl-av:synonym>has expected dividend date</fibo-fnd-utl-av:synonym>
	</owl:ObjectProperty>
	
	<owl:ObjectProperty rdf:about="&fibo-sec-eq-eq;hasFixedDividendRate">
		<rdfs:subPropertyOf rdf:resource="&lcc-lr;has"/>
		<rdfs:label>has fixed dividend rate</rdfs:label>
		<rdfs:domain rdf:resource="&fibo-sec-eq-eq;PreferredDividend"/>
		<rdfs:range rdf:resource="&fibo-fnd-acc-cur;PercentageMonetaryAmount"/>
		<skos:definition>indicates a pre-arranged fixed dividend rate, typically specified in the prospectus, for a preferred share</skos:definition>
	</owl:ObjectProperty>
	
	<owl:DatatypeProperty rdf:about="&fibo-sec-eq-eq;hasFloatingShares">
		<rdfs:subPropertyOf rdf:resource="&fibo-fnd-acc-cur;hasAmount"/>
		<rdfs:label xml:lang="en">has floating shares</rdfs:label>
		<rdfs:domain rdf:resource="&fibo-sec-eq-eq;EquityIssuer"/>
		<rdfs:range rdf:resource="&xsd;nonNegativeInteger"/>
		<skos:definition xml:lang="en">indicates the number of shares that are available for trading, i.e., the number of shares outstanding less closely held shares (those held by insiders) and restricted shares</skos:definition>
		<fibo-fnd-utl-av:explanatoryNote xml:lang="en">A relatively small float results in higher volatility, as a large purchase or sell order will have significant influence on the value of the stock.</fibo-fnd-utl-av:explanatoryNote>
	</owl:DatatypeProperty>
	
	<owl:ObjectProperty rdf:about="&fibo-sec-eq-eq;hasMinimumRedemptionPrice">
		<rdfs:subPropertyOf rdf:resource="&fibo-fnd-acc-cur;hasPrice"/>
		<rdfs:label>has minimum redemption price</rdfs:label>
		<rdfs:domain rdf:resource="&fibo-sec-eq-eq;EquityRedemptionProvision"/>
		<rdfs:range rdf:resource="&fibo-fnd-acc-cur;MonetaryAmount"/>
		<skos:definition>indicates the lowest market price above which a share may be redeemed</skos:definition>
	</owl:ObjectProperty>
	
	<owl:ObjectProperty rdf:about="&fibo-sec-eq-eq;hasRecordDate">
		<rdfs:subPropertyOf rdf:resource="&fibo-fnd-dt-fd;hasExplicitDate"/>
		<rdfs:label>has record date</rdfs:label>
		<rdfs:domain rdf:resource="&fibo-sec-eq-eq;Share"/>
		<rdfs:range rdf:resource="&fibo-fnd-dt-fd;ExplicitDate"/>
		<skos:definition>indicates the date on which the issuer checks to determine whether or not a party was on the company&apos;s books as a shareholder when required (i.e., they must have been on the books prior to the ex-dividend date), to identify who is eligible to receive the next dividend</skos:definition>
		<fibo-fnd-utl-av:adaptedFrom rdf:datatype="&xsd;anyURI">https://www.investor.gov/introduction-investing/investing-basics/glossary/ex-dividend-dates-when-are-you-entitled-stock-and</fibo-fnd-utl-av:adaptedFrom>
		<fibo-fnd-utl-av:explanatoryNote>Companies also use this date to determine who is sent proxy statements, financial reports, and other information.</fibo-fnd-utl-av:explanatoryNote>
		<fibo-fnd-utl-av:synonym>has date of record</fibo-fnd-utl-av:synonym>
	</owl:ObjectProperty>
	
	<owl:ObjectProperty rdf:about="&fibo-sec-eq-eq;hasRedemptionPremium">
		<rdfs:subPropertyOf rdf:resource="&fibo-fnd-acc-cur;hasPrice"/>
		<rdfs:label>has redemption premium</rdfs:label>
		<rdfs:domain rdf:resource="&fibo-sec-eq-eq;EquityRedemptionProvision"/>
		<rdfs:range rdf:resource="&fibo-fnd-acc-cur;MonetaryPrice"/>
		<skos:definition>indicates the premium price per share over the market price, if any, that must be paid in order to redeem the stock</skos:definition>
	</owl:ObjectProperty>
	
	<owl:DatatypeProperty rdf:about="&fibo-sec-eq-eq;hasShareClass">
		<rdfs:label xml:lang="en">has share class</rdfs:label>
		<rdfs:domain rdf:resource="&fibo-sec-eq-eq;Share"/>
		<rdfs:range rdf:resource="&xsd;string"/>
		<skos:definition xml:lang="en">indicates the class to which the share belongs, typically differentiated by privileges, such as voting rights</skos:definition>
		<fibo-fnd-utl-av:explanatoryNote xml:lang="en">Classes of shares, including shares in a mutual fund, are designated by name or a character (letter), such as A, B, C, etc.  In the case of a mutual fund, different classes of shares may incur different fees and expenses.</fibo-fnd-utl-av:explanatoryNote>
	</owl:DatatypeProperty>
	
	<owl:ObjectProperty rdf:about="&fibo-sec-eq-eq;hasSharePaymentStatus">
		<rdfs:subPropertyOf rdf:resource="&lcc-cr;isClassifiedBy"/>
		<rdfs:label xml:lang="en">has share payment status</rdfs:label>
		<rdfs:domain rdf:resource="&fibo-sec-eq-eq;Share"/>
		<rdfs:range rdf:resource="&fibo-sec-eq-eq;SharePaymentStatus"/>
		<skos:definition xml:lang="en">indicates the payment status for shares issued</skos:definition>
	</owl:ObjectProperty>
	
	<owl:DatatypeProperty rdf:about="&fibo-sec-eq-eq;hasSharesIssued">
		<rdfs:subPropertyOf rdf:resource="&fibo-fnd-acc-cur;hasAmount"/>
		<rdfs:label xml:lang="en">has shares issued</rdfs:label>
		<rdfs:domain rdf:resource="&fibo-sec-eq-eq;EquityIssuer"/>
		<rdfs:range rdf:resource="&xsd;nonNegativeInteger"/>
		<skos:definition xml:lang="en">indicates the number of shares authorized for sale by the board of directors, including shares sold to and held by shareholders as well as shares that are available for sale to generate capital, and shares available for distribution to insiders as part of their compensation packages</skos:definition>
	</owl:DatatypeProperty>
	
	<owl:DatatypeProperty rdf:about="&fibo-sec-eq-eq;hasSharesOutstanding">
		<rdfs:subPropertyOf rdf:resource="&fibo-fnd-acc-cur;hasAmount"/>
		<rdfs:label xml:lang="en">has shares outstanding</rdfs:label>
		<rdfs:domain rdf:resource="&fibo-sec-eq-eq;EquityIssuer"/>
		<rdfs:range rdf:resource="&xsd;nonNegativeInteger"/>
		<skos:definition xml:lang="en">indicates the number of shares currently held by shareholders, including those held by retail investors, institutional investors and insiders, and typically available for trading</skos:definition>
		<fibo-fnd-utl-av:explanatoryNote xml:lang="en">The number of outstanding shares is used in calculating key metrics such as a company&apos;s market capitalization, as well as its earnings per share (EPS) and cash flow per share (CFPS).</fibo-fnd-utl-av:explanatoryNote>
	</owl:DatatypeProperty>
	
	<owl:DatatypeProperty rdf:about="&fibo-sec-eq-eq;hasTreasuryShares">
		<rdfs:subPropertyOf rdf:resource="&fibo-fnd-acc-cur;hasAmount"/>
		<rdfs:label xml:lang="en">has treasury shares</rdfs:label>
		<rdfs:domain rdf:resource="&fibo-sec-eq-eq;EquityIssuer"/>
		<rdfs:range rdf:resource="&xsd;nonNegativeInteger"/>
		<skos:definition xml:lang="en">indicates the number of shares issued but not outstanding, including those that were available in the market at one time but have been repurchased by the company</skos:definition>
	</owl:DatatypeProperty>
	
	<owl:DatatypeProperty rdf:about="&fibo-sec-eq-eq;hasVotingRestriction">
		<rdfs:label xml:lang="en">has voting restriction</rdfs:label>
		<rdfs:domain rdf:resource="&fibo-sec-eq-eq;VotingRight"/>
		<rdfs:range rdf:resource="&xsd;string"/>
		<skos:definition>specifies restrictions on voting rights, if any</skos:definition>
		<fibo-fnd-utl-av:explanatoryNote>Such restrictions may apply regardless of the number of votes per share.</fibo-fnd-utl-av:explanatoryNote>
	</owl:DatatypeProperty>
	
	<owl:DatatypeProperty rdf:about="&fibo-sec-eq-eq;indicatesNumberOfShares">
		<rdfs:subPropertyOf rdf:resource="&fibo-fnd-acc-cur;hasAmount"/>
		<rdfs:label xml:lang="en">indicates number of shares</rdfs:label>
		<rdfs:domain rdf:resource="&fibo-sec-eq-eq;EquityPosition"/>
		<rdfs:range rdf:resource="&xsd;decimal"/>
		<skos:definition xml:lang="en">indicates the number of shares associated with the position</skos:definition>
	</owl:DatatypeProperty>
	
	<owl:DatatypeProperty rdf:about="&fibo-sec-eq-eq;isRedeemableAtIssuerOption">
		<rdfs:label>is redeemable at issuer option</rdfs:label>
		<rdfs:domain rdf:resource="&fibo-fbc-fi-fi;RedemptionProvision"/>
		<rdfs:range rdf:resource="&xsd;boolean"/>
		<skos:definition>indicates whether the issuer has the option of initiating the buy-back, similar to a call feature</skos:definition>
	</owl:DatatypeProperty>
	
	<owl:DatatypeProperty rdf:about="&fibo-sec-eq-eq;isRedeemableAtShareholderOption">
		<rdfs:label>is redeemable at shareholder option</rdfs:label>
		<rdfs:domain rdf:resource="&fibo-fbc-fi-fi;RedemptionProvision"/>
		<rdfs:range rdf:resource="&xsd;boolean"/>
		<skos:definition>indicates whether the shareholder has the option of initiating the buy-back, similar to a put feature</skos:definition>
	</owl:DatatypeProperty>
	
	<owl:ObjectProperty rdf:about="&fibo-sec-eq-eq;isSeniorTo">
		<rdf:type rdf:resource="&owl;TransitiveProperty"/>
		<rdfs:label>is senior to</rdfs:label>
		<rdfs:domain rdf:resource="&fibo-sec-eq-eq;Share"/>
		<rdfs:range rdf:resource="&fibo-sec-eq-eq;Share"/>
		<skos:definition>indicates that a given share (share class) has higher seniority than the related share, meaning that it gives the holder a higher claim on the assets of the issuer</skos:definition>
	</owl:ObjectProperty>
	
	<owl:ObjectProperty rdf:about="&fibo-sec-eq-eq;pays">
		<rdfs:label>pays</rdfs:label>
		<rdfs:domain rdf:resource="&fibo-sec-eq-eq;Share"/>
		<rdfs:range rdf:resource="&fibo-sec-eq-eq;Dividend"/>
		<skos:definition>relates a share to a dividend that it may pay to shareholders</skos:definition>
	</owl:ObjectProperty>
	
	<owl:ObjectProperty rdf:about="&fibo-sec-eq-eq;specifiesConversionDate">
		<rdfs:label>specifies conversion date</rdfs:label>
		<rdfs:domain rdf:resource="&fibo-sec-eq-eq;EquityConversionTerms"/>
		<rdfs:range rdf:resource="&fibo-fnd-dt-fd;Date"/>
		<skos:definition>indicates the date on which, or after which, conversion may occur</skos:definition>
	</owl:ObjectProperty>

</rdf:RDF>