<?xml version="1.0" encoding="UTF-8"?>
<!DOCTYPE rdf:RDF [
	<!ENTITY dct "http://purl.org/dc/terms/">
	<!ENTITY fibo-be-oac-exec "https://spec.edmcouncil.org/fibo/BE/OwnershipAndControl/Executives/">
	<!ENTITY fibo-fnd-acc-cur "https://spec.edmcouncil.org/fibo/FND/Accounting/CurrencyAmount/">
	<!ENTITY fibo-fnd-agr-ctr "https://spec.edmcouncil.org/fibo/FND/Agreements/Contracts/">
	<!ENTITY fibo-fnd-agrx-con "https://spec.edmcouncil.org/fibo/FND/AgreementsExt/ContractualConstructs/">
	<!ENTITY fibo-fnd-dt-fd "https://spec.edmcouncil.org/fibo/FND/DatesAndTimes/FinancialDates/">
	<!ENTITY fibo-fnd-tim-tim "https://spec.edmcouncil.org/fibo/FND/TimeExt/Time/">
	<!ENTITY fibo-fnd-utl-av "https://spec.edmcouncil.org/fibo/FND/Utilities/AnnotationVocabulary/">
	<!ENTITY fibo-fnd-utl-val "https://spec.edmcouncil.org/fibo/FND/Utilities/Values/">
	<!ENTITY fibo-md-eqx-pri "https://spec.edmcouncil.org/fibo/MD/EquityTemporal/EquityPricing/">
	<!ENTITY fibo-sec-dbt-bo-cft "https://spec.edmcouncil.org/fibo/SEC/Debt/Bonds/BondsCashflowTerms/">
	<!ENTITY fibo-sec-eq-eq "https://spec.edmcouncil.org/fibo/SEC/Equities/EquityInstruments/">
	<!ENTITY fibo-sec-eq-sha "https://spec.edmcouncil.org/fibo/SEC/Equities/ShareTerms/">
	<!ENTITY fibo-sec-eq-she "https://spec.edmcouncil.org/fibo/SEC/Equities/ShareholderEquity/">
	<!ENTITY fibo-sec-eq-shr "https://spec.edmcouncil.org/fibo/SEC/Equities/ShareholderRights/">
	<!ENTITY owl "http://www.w3.org/2002/07/owl#">
	<!ENTITY rdf "http://www.w3.org/1999/02/22-rdf-syntax-ns#">
	<!ENTITY rdfs "http://www.w3.org/2000/01/rdf-schema#">
	<!ENTITY skos "http://www.w3.org/2004/02/skos/core#">
	<!ENTITY xsd "http://www.w3.org/2001/XMLSchema#">
]>
<rdf:RDF
	xmlns:dct="http://purl.org/dc/terms/"
	xmlns:fibo-be-oac-exec="https://spec.edmcouncil.org/fibo/BE/OwnershipAndControl/Executives/"
	xmlns:fibo-fnd-acc-cur="https://spec.edmcouncil.org/fibo/FND/Accounting/CurrencyAmount/"
	xmlns:fibo-fnd-agr-ctr="https://spec.edmcouncil.org/fibo/FND/Agreements/Contracts/"
	xmlns:fibo-fnd-agrx-con="https://spec.edmcouncil.org/fibo/FND/AgreementsExt/ContractualConstructs/"
	xmlns:fibo-fnd-dt-fd="https://spec.edmcouncil.org/fibo/FND/DatesAndTimes/FinancialDates/"
	xmlns:fibo-fnd-tim-tim="https://spec.edmcouncil.org/fibo/FND/TimeExt/Time/"
	xmlns:fibo-fnd-utl-av="https://spec.edmcouncil.org/fibo/FND/Utilities/AnnotationVocabulary/"
	xmlns:fibo-fnd-utl-val="https://spec.edmcouncil.org/fibo/FND/Utilities/Values/"
	xmlns:fibo-md-eqx-pri="https://spec.edmcouncil.org/fibo/MD/EquityTemporal/EquityPricing/"
	xmlns:fibo-sec-dbt-bo-cft="https://spec.edmcouncil.org/fibo/SEC/Debt/Bonds/BondsCashflowTerms/"
	xmlns:fibo-sec-eq-eq="https://spec.edmcouncil.org/fibo/SEC/Equities/EquityInstruments/"
	xmlns:fibo-sec-eq-sha="https://spec.edmcouncil.org/fibo/SEC/Equities/ShareTerms/"
	xmlns:fibo-sec-eq-she="https://spec.edmcouncil.org/fibo/SEC/Equities/ShareholderEquity/"
	xmlns:fibo-sec-eq-shr="https://spec.edmcouncil.org/fibo/SEC/Equities/ShareholderRights/"
	xmlns:owl="http://www.w3.org/2002/07/owl#"
	xmlns:rdf="http://www.w3.org/1999/02/22-rdf-syntax-ns#"
	xmlns:rdfs="http://www.w3.org/2000/01/rdf-schema#"
	xmlns:skos="http://www.w3.org/2004/02/skos/core#"
	xmlns:xsd="http://www.w3.org/2001/XMLSchema#">
	
	<owl:Ontology rdf:about="https://spec.edmcouncil.org/fibo/SEC/Equities/ShareTerms/">
		<rdfs:label xml:lang="en">ShareTerms</rdfs:label>
		<dct:abstract>This ontology defines the kinds of terms that different clases of share may have, and that distinguish these from one another. These includes different combinations of voting rights, dividend terms, share coupons, participating and precedence terms as well as terms for convertible shares. This ontology also defines classes of share that are defined by differences in these rights and precedences, and the class of convertible shares.</dct:abstract>
		<owl:imports rdf:resource="http://www.w3.org/2004/02/skos/core"/>
		<owl:imports rdf:resource="https://spec.edmcouncil.org/fibo/BE/OwnershipAndControl/Executives/"/>
		<owl:imports rdf:resource="https://spec.edmcouncil.org/fibo/FBC/FinancialInstruments/FinancialInstruments/"/>
		<owl:imports rdf:resource="https://spec.edmcouncil.org/fibo/FND/Accounting/CurrencyAmount/"/>
		<owl:imports rdf:resource="https://spec.edmcouncil.org/fibo/FND/Agreements/Contracts/"/>
		<owl:imports rdf:resource="https://spec.edmcouncil.org/fibo/FND/AgreementsExt/ContractualConstructs/"/>
		<owl:imports rdf:resource="https://spec.edmcouncil.org/fibo/FND/DatesAndTimes/FinancialDates/"/>
		<owl:imports rdf:resource="https://spec.edmcouncil.org/fibo/FND/Relations/Relations/"/>
		<owl:imports rdf:resource="https://spec.edmcouncil.org/fibo/FND/TimeExt/Time/"/>
		<owl:imports rdf:resource="https://spec.edmcouncil.org/fibo/FND/Utilities/AnnotationVocabulary/"/>
		<owl:imports rdf:resource="https://spec.edmcouncil.org/fibo/FND/Utilities/Values/"/>
		<owl:imports rdf:resource="https://spec.edmcouncil.org/fibo/MD/EquityTemporal/EquityPricing/"/>
		<owl:imports rdf:resource="https://spec.edmcouncil.org/fibo/SEC/Debt/Bonds/BondsCashflowTerms/"/>
		<owl:imports rdf:resource="https://spec.edmcouncil.org/fibo/SEC/Equities/EquityInstruments/"/>
		<owl:imports rdf:resource="https://spec.edmcouncil.org/fibo/SEC/Equities/ShareholderEquity/"/>
		<owl:imports rdf:resource="https://spec.edmcouncil.org/fibo/SEC/Equities/ShareholderRights/"/>
		<owl:imports rdf:resource="https://spec.edmcouncil.org/fibo/SEC/SecuritiesExt/SchedulesExt/"/>
		<owl:imports rdf:resource="https://spec.edmcouncil.org/fibo/SEC/SecuritiesExt/SecuritiesListingsExt/"/>
		<owl:versionIRI rdf:resource="https://spec.edmcouncil.org/fibo/SEC/Equities/ShareTerms/"/>
		<fibo-fnd-utl-av:hasMaturityLevel rdf:resource="&fibo-fnd-utl-av;Provisional"/>
	</owl:Ontology>
	
	<owl:Class rdf:about="&fibo-be-oac-exec;ArticlesOfIncorporation">
		<rdfs:subClassOf>
			<owl:Restriction>
				<owl:onProperty rdf:resource="&fibo-sec-eq-sha;setsOut"/>
				<owl:someValuesFrom rdf:resource="&fibo-sec-eq-sha;CompanyEquityTermsSet"/>
			</owl:Restriction>
		</rdfs:subClassOf>
		<skos:definition xml:lang="en">proxy</skos:definition>
	</owl:Class>
	
	<owl:Class rdf:about="&fibo-sec-eq-sha;CompanyEquityTermsSet">
		<rdfs:subClassOf rdf:resource="&fibo-fnd-agr-ctr;ContractualCommitment"/>
		<rdfs:label xml:lang="en">company equity terms</rdfs:label>
		<skos:definition xml:lang="en">Terms setting out the equity in a company, including the various kinds of rights, the shares that embody those rights etc.</skos:definition>
	</owl:Class>
	
	<owl:Class rdf:about="&fibo-sec-eq-sha;ConvertibleCommonShare">
		<rdfs:subClassOf rdf:resource="&fibo-sec-eq-sha;ConvertibleShare"/>
		<rdfs:subClassOf rdf:resource="&fibo-sec-eq-sha;OrdinaryShare"/>
		<rdfs:label xml:lang="en">convertible common share</rdfs:label>
		<owl:disjointWith rdf:resource="&fibo-sec-eq-sha;ConvertiblePreferenceShare"/>
	</owl:Class>
	
	<owl:Class rdf:about="&fibo-sec-eq-sha;ConvertibleIntoFacet">
		<rdfs:label xml:lang="en">convertible into facet</rdfs:label>
	</owl:Class>
	
	<owl:Class rdf:about="&fibo-sec-eq-sha;ConvertibleIntoFacet.1">
		<rdfs:label xml:lang="en">ConvertibleIntoFacet.1</rdfs:label>
	</owl:Class>
	
	<owl:Class rdf:about="&fibo-sec-eq-sha;ConvertibleParticipatingPreferenceShare">
		<rdfs:subClassOf rdf:resource="&fibo-sec-eq-sha;ConvertiblePreferenceShare"/>
		<rdfs:subClassOf rdf:resource="&fibo-sec-eq-sha;ParticipatingPreferenceShare"/>
		<rdfs:label xml:lang="en">convertible participating preference share</rdfs:label>
		<skos:definition xml:lang="en">A preference share that can be converted into common shares at a fixed conversion price. Preference or preferred shares entitle a holder to a prior claim on any dividend paid by the company before payment is made on ordinary shares.</skos:definition>
	</owl:Class>
	
	<owl:Class rdf:about="&fibo-sec-eq-sha;ConvertiblePreferenceShare">
		<rdfs:subClassOf rdf:resource="&fibo-sec-eq-sha;ConvertibleShare"/>
		<rdfs:subClassOf rdf:resource="&fibo-sec-eq-sha;PreferenceShare"/>
		<rdfs:subClassOf>
			<owl:Restriction>
				<owl:onProperty rdf:resource="&fibo-sec-eq-sha;convertibleInto"/>
				<owl:someValuesFrom rdf:resource="&fibo-sec-eq-eq;PubliclyTradedShare"/>
			</owl:Restriction>
		</rdfs:subClassOf>
		<rdfs:label xml:lang="en">convertible preference share</rdfs:label>
		<skos:definition xml:lang="en">A Preferred Share which is convertible into another security.</skos:definition>
	</owl:Class>
	
	<owl:Class rdf:about="&fibo-sec-eq-sha;ConvertibleShare">
		<rdfs:subClassOf rdf:resource="&fibo-sec-eq-eq;Share"/>
		<rdfs:subClassOf>
			<owl:Restriction>
				<owl:onProperty rdf:resource="&fibo-sec-eq-sha;convertibleInto"/>
				<owl:someValuesFrom rdf:resource="https://spec.edmcouncil.org/fibo/FBC/FinancialInstruments/FinancialInstruments/Security"/>
			</owl:Restriction>
		</rdfs:subClassOf>
		<rdfs:subClassOf>
			<owl:Restriction>
				<owl:onProperty rdf:resource="&fibo-sec-eq-sha;hasConversionTerms"/>
				<owl:someValuesFrom rdf:resource="&fibo-sec-eq-sha;EquityConversionTerms"/>
			</owl:Restriction>
		</rdfs:subClassOf>
		<rdfs:label xml:lang="en">convertible share</rdfs:label>
		<skos:definition xml:lang="en">A Share which is convertible into another security, usually a share in the same company.</skos:definition>
	</owl:Class>
	
	<owl:Class rdf:about="&fibo-sec-eq-sha;CumulativeFacet">
		<rdfs:label xml:lang="en">cumulative facet</rdfs:label>
	</owl:Class>
	
	<owl:Class rdf:about="&fibo-sec-eq-sha;CumulativeFacet.1">
		<rdfs:label xml:lang="en">CumulativeFacet.1</rdfs:label>
	</owl:Class>
	
	<owl:Class rdf:about="&fibo-sec-eq-sha;CumulativePreferenceShare">
		<rdfs:subClassOf rdf:resource="&fibo-sec-eq-sha;PreferenceShare"/>
		<rdfs:label xml:lang="en">cumulative preference share</rdfs:label>
		<owl:disjointWith rdf:resource="&fibo-sec-eq-sha;NonCumulativePreferenceShare"/>
	</owl:Class>
	
	<owl:Class rdf:about="&fibo-sec-eq-sha;DividendTerms">
		<rdfs:subClassOf rdf:resource="&fibo-sec-eq-sha;CompanyEquityTermsSet"/>
		<rdfs:subClassOf>
			<owl:Restriction>
				<owl:onProperty rdf:resource="&fibo-sec-eq-sha;hasDistributionMethod"/>
				<owl:onClass rdf:resource="&fibo-sec-eq-eq;DividendsDistributionMethod"/>
				<owl:maxQualifiedCardinality rdf:datatype="&xsd;nonNegativeInteger">1</owl:maxQualifiedCardinality>
			</owl:Restriction>
		</rdfs:subClassOf>
		<rdfs:label xml:lang="en">dividend terms</rdfs:label>
	</owl:Class>
	
	<owl:Class rdf:about="&fibo-sec-eq-sha;EquityConversionTerms">
		<rdfs:subClassOf rdf:resource="&fibo-sec-eq-sha;CompanyEquityTermsSet"/>
		<rdfs:subClassOf rdf:resource="https://spec.edmcouncil.org/fibo/SEC/Securities/SecuritiesIssuance/ConversionTerms"/>
		<rdfs:subClassOf>
			<owl:Restriction>
				<owl:onProperty rdf:resource="https://spec.edmcouncil.org/fibo/SEC/Securities/SecuritiesIssuance/specifiesConversionInto"/>
				<owl:someValuesFrom rdf:resource="https://spec.edmcouncil.org/fibo/FBC/FinancialInstruments/FinancialInstruments/Security"/>
			</owl:Restriction>
		</rdfs:subClassOf>
		<rdfs:label xml:lang="en">equity conversion terms</rdfs:label>
		<skos:definition xml:lang="en">Contractual specifications when an Equity security can be converted to another security (usually of the same issuer).</skos:definition>
	</owl:Class>
	
	<owl:Class rdf:about="&fibo-sec-eq-sha;EquityListing">
		<rdfs:subClassOf rdf:resource="https://spec.edmcouncil.org/fibo/SEC/Securities/SecuritiesListings/SecurityListing"/>
		<rdfs:label xml:lang="en">equity listing</rdfs:label>
		<skos:definition xml:lang="en">The listing of an equity security (stock) on an equities exchange or multilateral trading facility.</skos:definition>
		<fibo-fnd-utl-av:explanatoryNote xml:lang="en">This is not the security or the exchange but the listing of the security on the exchange. Facts defined for Equity Listing are facts about that security listed on that exchange or trading facility.</fibo-fnd-utl-av:explanatoryNote>
	</owl:Class>
	
	<owl:Class rdf:about="&fibo-sec-eq-sha;NonCumulativePreferenceShare">
		<rdfs:subClassOf rdf:resource="&fibo-sec-eq-sha;PreferenceShare"/>
		<rdfs:label xml:lang="en">non cumulative preference share</rdfs:label>
		<skos:definition xml:lang="en">Non Cumulative Preference Shares are preference shares where the payment of the fixed dividend, if not made in a given trading year, is not carried forward to the next trading year.</skos:definition>
		<fibo-fnd-utl-av:explanatoryNote xml:lang="en">All preference shares are either cumulative or non cumulative.</fibo-fnd-utl-av:explanatoryNote>
	</owl:Class>
	
	<owl:Class rdf:about="&fibo-sec-eq-sha;NonParticipatingPreferenceShare">
		<rdfs:subClassOf rdf:resource="&fibo-sec-eq-sha;NonParticipatingShare"/>
		<rdfs:subClassOf rdf:resource="&fibo-sec-eq-sha;PreferenceShare"/>
		<rdfs:label xml:lang="en">non participating preference share</rdfs:label>
		<skos:definition xml:lang="en">The usual type of preference share, which is not a Participating Preference Share</skos:definition>
	</owl:Class>
	
	<owl:Class rdf:about="&fibo-sec-eq-sha;NonParticipatingShare">
		<rdfs:subClassOf rdf:resource="&fibo-sec-eq-eq;Share"/>
		<rdfs:label xml:lang="en">non participating share</rdfs:label>
		<owl:disjointWith rdf:resource="&fibo-sec-eq-sha;ParticipatingShare"/>
	</owl:Class>
	
	<owl:Class rdf:about="&fibo-sec-eq-sha;OneVotePerHolder">
		<rdfs:subClassOf rdf:resource="&fibo-sec-eq-sha;RestrictedVotingRight"/>
		<rdfs:label xml:lang="en">one vote per holder</rdfs:label>
		<skos:definition xml:lang="en">Voting rights limited rights to one vote per person, or institution, to avoid any party taking control. Further notes: Not in ISO FIBIM selection. Identified from new article on UK building societies. Note that further types of voting rights can be defined any time in the prospectus for a new security. Original Article quotation: &quot;Adrian Coles, director general of the Building Societies Association, said it would be helpful if building societies could issue shares to investors to raise funds, but limit voting rights to one vote per person, or institution, to avoid any party taking control. Article Source:article on Profit Participating Deferred Shares in relation to West Bromwich Building society By Philip Aldrick,[citation missing], 12 June 2009</skos:definition>
	</owl:Class>
	
	<owl:Class rdf:about="&fibo-sec-eq-sha;OrdinaryDividendTerms">
		<rdfs:subClassOf rdf:resource="&fibo-fnd-agr-ctr;NonBindingTerms"/>
		<rdfs:subClassOf rdf:resource="&fibo-sec-eq-sha;DividendTerms"/>
		<rdfs:subClassOf>
			<owl:Restriction>
				<owl:onProperty rdf:resource="&fibo-sec-eq-sha;dividendPaymentDate"/>
				<owl:onClass rdf:resource="&fibo-fnd-utl-val;DayMonthValue"/>
				<owl:maxQualifiedCardinality rdf:datatype="&xsd;nonNegativeInteger">12</owl:maxQualifiedCardinality>
			</owl:Restriction>
		</rdfs:subClassOf>
		<rdfs:subClassOf>
			<owl:Restriction>
				<owl:onProperty rdf:resource="&fibo-sec-eq-sha;dividendPaymentDate"/>
				<owl:onClass rdf:resource="&fibo-fnd-utl-val;DayMonthValue"/>
				<owl:minQualifiedCardinality rdf:datatype="&xsd;nonNegativeInteger">1</owl:minQualifiedCardinality>
			</owl:Restriction>
		</rdfs:subClassOf>
		<rdfs:label xml:lang="en">ordinary dividend terms</rdfs:label>
		<skos:definition xml:lang="en">Formal terms about the Dividend payments on an Ordinary Share.</skos:definition>
		<fibo-fnd-utl-av:explanatoryNote xml:lang="en">These are terms that are not contractually binding on the company.</fibo-fnd-utl-av:explanatoryNote>
	</owl:Class>
	
	<owl:Class rdf:about="&fibo-sec-eq-sha;OrdinaryShare">
		<rdfs:subClassOf rdf:resource="&fibo-sec-eq-eq;Share"/>
		<rdfs:subClassOf>
			<owl:Restriction>
				<owl:onProperty rdf:resource="&fibo-sec-eq-sha;pays"/>
				<owl:someValuesFrom rdf:resource="&fibo-md-eqx-pri;OrdinaryShareDividend"/>
			</owl:Restriction>
		</rdfs:subClassOf>
		<rdfs:subClassOf>
			<owl:Restriction>
				<owl:onProperty rdf:resource="&fibo-sec-eq-she;confersOwnershipOf"/>
				<owl:someValuesFrom rdf:resource="&fibo-sec-eq-she;JuniorEquity"/>
			</owl:Restriction>
		</rdfs:subClassOf>
		<rdfs:label xml:lang="en">ordinary share</rdfs:label>
		<owl:disjointWith rdf:resource="&fibo-sec-eq-sha;PreferenceShare"/>
		<skos:definition xml:lang="en">A security that represents ownership in a corporation. Holders of common share exercise control by electing a board of directors and voting on corporate policy.</skos:definition>
		<fibo-fnd-utl-av:explanatoryNote xml:lang="en">Common stockholders are on the bottom of the priority ladder for ownership structure. In the event of liquidation, common shareholders have rights to a company&apos;s assets only after bondholders, preferred shareholders and other debtholders have been paid in full.</fibo-fnd-utl-av:explanatoryNote>
	</owl:Class>
	
	<owl:Class rdf:about="&fibo-sec-eq-sha;ParticipatingFacet">
		<rdfs:label xml:lang="en">participating facet</rdfs:label>
	</owl:Class>
	
	<owl:Class rdf:about="&fibo-sec-eq-sha;ParticipatingFacet.1">
		<rdfs:label xml:lang="en">ParticipatingFacet.1</rdfs:label>
	</owl:Class>
	
	<owl:Class rdf:about="&fibo-sec-eq-sha;ParticipatingPreferenceShare">
		<rdfs:subClassOf rdf:resource="&fibo-sec-eq-sha;ParticipatingShare"/>
		<rdfs:subClassOf rdf:resource="&fibo-sec-eq-sha;PreferenceShare"/>
		<rdfs:subClassOf>
			<owl:Restriction>
				<owl:onProperty rdf:resource="&fibo-sec-eq-sha;optionallyPays"/>
				<owl:onClass rdf:resource="&fibo-md-eqx-pri;OrdinaryShareDividend"/>
				<owl:maxQualifiedCardinality rdf:datatype="&xsd;nonNegativeInteger">1</owl:maxQualifiedCardinality>
			</owl:Restriction>
		</rdfs:subClassOf>
		<rdfs:subClassOf>
			<owl:Restriction>
				<owl:onProperty rdf:resource="&fibo-sec-eq-sha;participatingPreferenceShareSeniorToPreferenceShare"/>
				<owl:someValuesFrom rdf:resource="&fibo-sec-eq-sha;PreferenceShare"/>
			</owl:Restriction>
		</rdfs:subClassOf>
		<rdfs:label xml:lang="en">participating preference share</rdfs:label>
		<skos:definition xml:lang="en">Like the preferred shares, participating preference shares have a prior claim on dividends, and on assets in an event of corporate liquidation or dissolution. But preferred stock would take precedence over preference stock in respect of dividends and assets that may be available for distribution.</skos:definition>
	</owl:Class>
	
	<owl:Class rdf:about="&fibo-sec-eq-sha;ParticipatingShare">
		<rdfs:subClassOf rdf:resource="&fibo-sec-eq-eq;Share"/>
		<rdfs:label xml:lang="en">participating share</rdfs:label>
	</owl:Class>
	
	<owl:Class rdf:about="&fibo-sec-eq-sha;PrecedenceRight">
		<rdfs:subClassOf rdf:resource="&fibo-fnd-agrx-con;ContractualRight"/>
		<rdfs:label xml:lang="en">precedence right</rdfs:label>
		<skos:definition xml:lang="en">The rights of various parties in respect of the assets of some entity in the event of that entity being wound up.</skos:definition>
		<fibo-fnd-utl-av:explanatoryNote xml:lang="en">Some of these rights are enshrined in law. A special case of these is shareholder rights which are defined, for different classes of equity, by the Company Articles of Association or equivalent Documentation. These are the rights defined in the Equity Priority Terms Set.</fibo-fnd-utl-av:explanatoryNote>
	</owl:Class>
	
	<owl:Class rdf:about="&fibo-sec-eq-sha;PreferenceShare">
		<rdfs:subClassOf rdf:resource="&fibo-sec-eq-eq;Share"/>
		<rdfs:subClassOf>
			<owl:Restriction>
				<owl:onProperty rdf:resource="&fibo-sec-eq-sha;hasCoupon"/>
				<owl:someValuesFrom>
					<owl:Class>
						<owl:unionOf rdf:parseType="Collection">
							<rdf:Description rdf:about="&fibo-md-eqx-pri;OrdinaryShareDividend">
							</rdf:Description>
							<rdf:Description rdf:about="&fibo-md-eqx-pri;PreferenceShareCoupon">
							</rdf:Description>
						</owl:unionOf>
					</owl:Class>
				</owl:someValuesFrom>
			</owl:Restriction>
		</rdfs:subClassOf>
		<rdfs:subClassOf>
			<owl:Restriction>
				<owl:onProperty rdf:resource="&fibo-sec-eq-sha;mayConfer"/>
				<owl:someValuesFrom rdf:resource="&fibo-sec-eq-shr;ExtraordinaryVotingRight"/>
			</owl:Restriction>
		</rdfs:subClassOf>
		<rdfs:subClassOf>
			<owl:Restriction>
				<owl:onProperty rdf:resource="&fibo-sec-eq-sha;preferenceShareSeniorToOrdinaryShare"/>
				<owl:someValuesFrom rdf:resource="&fibo-sec-eq-sha;OrdinaryShare"/>
			</owl:Restriction>
		</rdfs:subClassOf>
		<rdfs:subClassOf>
			<owl:Restriction>
				<owl:onProperty rdf:resource="&fibo-sec-eq-she;confersOwnershipOf.1"/>
				<owl:someValuesFrom rdf:resource="&fibo-sec-eq-she;SeniorEquity"/>
			</owl:Restriction>
		</rdfs:subClassOf>
		<rdfs:label xml:lang="en">preference share</rdfs:label>
	</owl:Class>
	
	<owl:Class rdf:about="&fibo-sec-eq-sha;PreferredCouponPaymentTermSet">
		<rdfs:subClassOf rdf:resource="&fibo-sec-eq-sha;DividendTerms"/>
		<rdfs:subClassOf>
			<owl:Restriction>
				<owl:onProperty rdf:resource="&fibo-sec-eq-sha;includesScheduleTerm"/>
				<owl:someValuesFrom rdf:resource="&fibo-sec-eq-sha;ShareCouponSchedule"/>
			</owl:Restriction>
		</rdfs:subClassOf>
		<rdfs:label xml:lang="en">preferred coupon payment term set</rdfs:label>
		<skos:definition xml:lang="en">Terms for payment of a Dividend on a Preferred Stock.</skos:definition>
		<fibo-fnd-utl-av:explanatoryNote xml:lang="en">These, like the Dividend terms, are not contractually binding terms; the dividend is paid at the discretion of the company but takes precedence over the ordinary share dividend.</fibo-fnd-utl-av:explanatoryNote>
	</owl:Class>
	
	<owl:Class rdf:about="&fibo-sec-eq-sha;RestrictedVotingRight">
		<rdfs:subClassOf rdf:resource="&fibo-sec-eq-eq;VotingRight"/>
		<rdfs:label xml:lang="en">restricted voting right</rdfs:label>
		<skos:definition xml:lang="en">Restricted Voting. The holder has the right to vote but there are restrictions on these rights.</skos:definition>
		<fibo-fnd-utl-av:explanatoryNote xml:lang="en">The restrictions are described in a separate term about the Voting rights.</fibo-fnd-utl-av:explanatoryNote>
	</owl:Class>
	
	<owl:Class rdf:about="&fibo-sec-eq-sha;ShareCouponSchedule">
		<rdfs:label xml:lang="en">share coupon schedule</rdfs:label>
	</owl:Class>
	
	<owl:Class rdf:about="&fibo-sec-eq-sha;ShareCouponScheduleSpecification">
		<rdfs:subClassOf rdf:resource="&fibo-sec-dbt-bo-cft;CouponScheduleSpecification"/>
		<rdfs:subClassOf>
			<owl:Restriction>
				<owl:onProperty rdf:resource="&fibo-md-eqx-pri;scheduledDividendPayment"/>
				<owl:someValuesFrom rdf:resource="&fibo-md-eqx-pri;EquityDividendPayment"/>
			</owl:Restriction>
		</rdfs:subClassOf>
		<rdfs:label xml:lang="en">share coupon schedule specification</rdfs:label>
		<skos:definition xml:lang="en">Schedule of dates on which a Share Coupon Payment is to take place.</skos:definition>
		<skos:editorialNote xml:lang="en">At present it is assumed that this has all and only the same sceduleing specification terms as for debt coupon payment events.</skos:editorialNote>
	</owl:Class>
	
	<owl:Class rdf:about="&fibo-sec-eq-sha;ShareholderPrecedenceRightsFacet">
		<rdfs:label xml:lang="en">shareholder precedence rights facet</rdfs:label>
		<skos:definition xml:lang="en">Facet based on the class or seniority of the equity represented by the shares i.e. ordinary, preference and so on.</skos:definition>
	</owl:Class>
	
	<owl:Class rdf:about="&fibo-sec-eq-sha;ShareholderPrecedenceRightsFacet.1">
		<rdfs:label xml:lang="en">ShareholderPrecedenceRightsFacet.1</rdfs:label>
	</owl:Class>
	
	<owl:Class rdf:about="&fibo-sec-eq-sha;SubordinatedVotingRight">
		<rdfs:subClassOf rdf:resource="&fibo-sec-eq-eq;VotingRight"/>
		<rdfs:label xml:lang="en">subordinated voting right</rdfs:label>
		<skos:definition xml:lang="en">Subordinated Voting. Action: this is a self-referential non definition, from ISO FIBIM.</skos:definition>
	</owl:Class>
	
	<owl:DatatypeProperty rdf:about="&fibo-sec-eq-sha;autoReinvestment">
		<rdfs:label xml:lang="en">auto reinvestment</rdfs:label>
		<rdfs:domain rdf:resource="&fibo-sec-eq-sha;DividendTerms"/>
		<rdfs:range rdf:resource="&xsd;boolean"/>
		<skos:definition xml:lang="en">Whether the security provides for mandatorily &amp;amp; automatically re-investing the dividend from that security towards buying more of the same security.</skos:definition>
	</owl:DatatypeProperty>
	
	<owl:ObjectProperty rdf:about="&fibo-sec-eq-sha;conversionDate">
		<rdfs:label xml:lang="en">conversion date</rdfs:label>
		<rdfs:domain rdf:resource="&fibo-sec-eq-sha;EquityConversionTerms"/>
		<rdfs:range rdf:resource="&fibo-fnd-dt-fd;Date"/>
		<skos:definition xml:lang="en">Date on or after which the specified conversion may take place.</skos:definition>
	</owl:ObjectProperty>
	
	<owl:ObjectProperty rdf:about="&fibo-sec-eq-sha;convertibleInto">
		<rdfs:label xml:lang="en">convertible into</rdfs:label>
		<rdfs:domain rdf:resource="&fibo-sec-eq-sha;ConvertibleShare"/>
		<rdfs:range rdf:resource="https://spec.edmcouncil.org/fibo/FBC/FinancialInstruments/FinancialInstruments/Security"/>
		<skos:definition xml:lang="en">The security into which the convertible share can be converted. It is assumed this can be any tradable security.</skos:definition>
	</owl:ObjectProperty>
	
	<owl:DatatypeProperty rdf:about="&fibo-sec-eq-sha;cumulative">
		<rdfs:label xml:lang="en">cumulative</rdfs:label>
		<rdfs:domain rdf:resource="&fibo-sec-eq-sha;CumulativePreferenceShare"/>
		<rdfs:range rdf:resource="&xsd;boolean"/>
		<skos:definition xml:lang="en">Whether or not the payment of the fixed dividend, if not made in a given trading year, is carried forward to the next trading year. This is no: skipped payments are not carried forward.</skos:definition>
	</owl:DatatypeProperty>
	
	<owl:DatatypeProperty rdf:about="&fibo-sec-eq-sha;cumulative.1">
		<rdfs:label xml:lang="en">cumulative</rdfs:label>
		<rdfs:domain rdf:resource="&fibo-sec-eq-sha;NonCumulativePreferenceShare"/>
		<rdfs:range rdf:resource="&xsd;boolean"/>
		<skos:definition xml:lang="en">Whether or not the payment of the fixed dividend, if not made in a given trading year, is carried forward to the next trading year. This is yes: skipped dividend payments are accumulated until they are finally paid.</skos:definition>
	</owl:DatatypeProperty>
	
	<owl:DatatypeProperty rdf:about="&fibo-sec-eq-sha;cumulative.2">
		<rdfs:label xml:lang="en">cumulative</rdfs:label>
		<rdfs:domain rdf:resource="&fibo-sec-eq-sha;PreferenceShare"/>
		<rdfs:range rdf:resource="&xsd;boolean"/>
		<skos:definition xml:lang="en">Whether or not the payment of the fixed dividend, if not made in a given trading year, is carried forward to the next trading year. If yes, skipped dividend payments are accumulated until they are finally paid. If no, skipped payments are not carried forward.</skos:definition>
	</owl:DatatypeProperty>
	
	<owl:ObjectProperty rdf:about="&fibo-sec-eq-sha;dividendAmount">
		<rdfs:label xml:lang="en">dividend amount</rdfs:label>
		<rdfs:domain rdf:resource="&fibo-sec-eq-sha;PreferredCouponPaymentTermSet"/>
		<rdfs:range rdf:resource="&fibo-fnd-acc-cur;MonetaryAmount"/>
		<skos:definition xml:lang="en">Planned dividend amount for preferred shares</skos:definition>
	</owl:ObjectProperty>
	
	<owl:ObjectProperty rdf:about="&fibo-sec-eq-sha;dividendDate">
		<rdfs:label xml:lang="en">dividend date</rdfs:label>
		<rdfs:domain rdf:resource="&fibo-sec-eq-sha;PreferredCouponPaymentTermSet"/>
		<rdfs:range rdf:resource="&fibo-fnd-utl-val;DayMonthValue"/>
		<skos:definition xml:lang="en">Planned dividend date (day and month) for regular dividend payment commitment.</skos:definition>
	</owl:ObjectProperty>
	
	<owl:ObjectProperty rdf:about="&fibo-sec-eq-sha;dividendExDate">
		<rdfs:label xml:lang="en">dividend ex date</rdfs:label>
		<rdfs:domain rdf:resource="&fibo-sec-eq-sha;DividendTerms"/>
		<rdfs:range rdf:resource="&fibo-fnd-utl-val;DayMonthValue"/>
		<skos:definition xml:lang="en">The day and month on which the security is traded &quot;Ex Dividend&quot;.</skos:definition>
	</owl:ObjectProperty>
	
	<owl:ObjectProperty rdf:about="&fibo-sec-eq-sha;dividendPaymentDate">
		<rdfs:subPropertyOf rdf:resource="&fibo-fnd-agr-ctr;isQualifiedBy"/>
		<rdfs:label xml:lang="en">dividend payment date</rdfs:label>
		<rdfs:domain rdf:resource="&fibo-sec-eq-sha;OrdinaryDividendTerms"/>
		<rdfs:range rdf:resource="&fibo-fnd-utl-val;DayMonthValue"/>
		<skos:definition xml:lang="en">The day and month on which dividends are to be paid.</skos:definition>
	</owl:ObjectProperty>
	
	<owl:ObjectProperty rdf:about="&fibo-sec-eq-sha;dividendPaymentFrequency">
		<rdfs:label xml:lang="en">dividend payment frequency</rdfs:label>
		<rdfs:domain rdf:resource="&fibo-sec-eq-sha;DividendTerms"/>
		<rdfs:range rdf:resource="&fibo-fnd-tim-tim;Frequency"/>
		<skos:definition xml:lang="en">The frequency with which dividends are expected to be paid out.</skos:definition>
	</owl:ObjectProperty>
	
	<owl:ObjectProperty rdf:about="&fibo-sec-eq-sha;dividendRate">
		<rdfs:label xml:lang="en">dividend rate</rdfs:label>
		<rdfs:domain rdf:resource="&fibo-sec-eq-sha;PreferredCouponPaymentTermSet"/>
		<rdfs:range rdf:resource="&fibo-fnd-utl-val;PercentageValue"/>
		<skos:definition xml:lang="en">Planned dividend rate, for preferred shares.</skos:definition>
	</owl:ObjectProperty>
	
	<owl:ObjectProperty rdf:about="&fibo-sec-eq-sha;gracePeriod">
		<rdfs:label xml:lang="en">grace period</rdfs:label>
		<rdfs:domain rdf:resource="&fibo-sec-eq-sha;PreferredCouponPaymentTermSet"/>
		<rdfs:range rdf:resource="&fibo-fnd-tim-tim;Duration"/>
	</owl:ObjectProperty>
	
	<owl:ObjectProperty rdf:about="&fibo-sec-eq-sha;hasConversionTerms">
		<rdfs:subPropertyOf rdf:resource="&fibo-fnd-agr-ctr;hasContractualElement"/>
		<rdfs:label xml:lang="en">has conversion terms</rdfs:label>
		<rdfs:domain rdf:resource="&fibo-sec-eq-sha;ConvertibleShare"/>
		<rdfs:range rdf:resource="&fibo-sec-eq-sha;EquityConversionTerms"/>
	</owl:ObjectProperty>
	
	<owl:ObjectProperty rdf:about="&fibo-sec-eq-sha;hasCoupon">
		<rdfs:label xml:lang="en">has coupon</rdfs:label>
		<rdfs:domain rdf:resource="&fibo-sec-eq-sha;PreferenceShare"/>
		<rdfs:range>
			<owl:Class>
				<owl:unionOf rdf:parseType="Collection">
					<rdf:Description rdf:about="&fibo-md-eqx-pri;OrdinaryShareDividend">
					</rdf:Description>
					<rdf:Description rdf:about="&fibo-md-eqx-pri;PreferenceShareCoupon">
					</rdf:Description>
				</owl:unionOf>
			</owl:Class>
		</rdfs:range>
	</owl:ObjectProperty>
	
	<owl:ObjectProperty rdf:about="&fibo-sec-eq-sha;hasDistributionMethod">
		<rdfs:label xml:lang="en">has distribution method</rdfs:label>
		<rdfs:domain rdf:resource="&fibo-sec-eq-sha;DividendTerms"/>
		<rdfs:range rdf:resource="&fibo-sec-eq-eq;DividendsDistributionMethod"/>
		<skos:definition xml:lang="en">Method by which Dividend payments are to be distributed.</skos:definition>
	</owl:ObjectProperty>
	
	<owl:ObjectProperty rdf:about="&fibo-sec-eq-sha;hasListing">
		<rdfs:label>has listing</rdfs:label>
	</owl:ObjectProperty>
	
	<owl:ObjectProperty rdf:about="&fibo-sec-eq-sha;includesScheduleTerm">
		<rdfs:label xml:lang="en">includes schedule term</rdfs:label>
		<rdfs:domain rdf:resource="&fibo-sec-eq-sha;PreferredCouponPaymentTermSet"/>
		<rdfs:range rdf:resource="&fibo-sec-eq-sha;ShareCouponSchedule"/>
	</owl:ObjectProperty>
	
	<owl:ObjectProperty rdf:about="&fibo-sec-eq-sha;isSeniorToAClassOfOrdinaryShare">
		<rdfs:subPropertyOf rdf:resource="&fibo-sec-eq-eq;isSeniorTo"/>
		<rdfs:label xml:lang="en">is senior to a class of ordinary share</rdfs:label>
		<rdfs:domain rdf:resource="&fibo-sec-eq-sha;OrdinaryShare"/>
		<rdfs:range rdf:resource="&fibo-sec-eq-sha;OrdinaryShare"/>
	</owl:ObjectProperty>
	
	<owl:ObjectProperty rdf:about="&fibo-sec-eq-sha;isSeniorToAClassOfPreferenceShare">
		<rdfs:subPropertyOf rdf:resource="&fibo-sec-eq-eq;isSeniorTo"/>
		<rdfs:label xml:lang="en">is senior to a class of preference share</rdfs:label>
		<rdfs:domain rdf:resource="&fibo-sec-eq-sha;PreferenceShare"/>
		<rdfs:range rdf:resource="&fibo-sec-eq-sha;PreferenceShare"/>
	</owl:ObjectProperty>
	
	<owl:ObjectProperty rdf:about="&fibo-sec-eq-sha;maturityDate">
		<rdfs:label xml:lang="en">maturity date</rdfs:label>
		<rdfs:domain rdf:resource="&fibo-sec-eq-sha;ParticipatingShare"/>
		<rdfs:range rdf:resource="&fibo-fnd-dt-fd;Date"/>
		<skos:definition xml:lang="en">Date/time at which the security will no longer exist, eg, redeemable preference shares. Definition:FIBIM</skos:definition>
	</owl:ObjectProperty>
	
	<owl:ObjectProperty rdf:about="&fibo-sec-eq-sha;maturityDate.1">
		<rdfs:label xml:lang="en">maturity date</rdfs:label>
		<rdfs:domain rdf:resource="&fibo-sec-eq-sha;PreferenceShare"/>
		<rdfs:range rdf:resource="&fibo-fnd-dt-fd;Date"/>
		<skos:definition xml:lang="en">Date/time at which the security will no longer exist, eg, redeemable preference shares. Definition:FIBIM</skos:definition>
	</owl:ObjectProperty>
	
	<owl:ObjectProperty rdf:about="&fibo-sec-eq-sha;mayConfer">
		<rdfs:label xml:lang="en">may confer</rdfs:label>
		<rdfs:domain rdf:resource="&fibo-sec-eq-sha;PreferenceShare"/>
		<rdfs:range rdf:resource="&fibo-sec-eq-shr;ExtraordinaryVotingRight"/>
		<skos:definition xml:lang="en">The right of the holder of the Preference Shares to vote on matters affecting the business of the issuing company. A preference share may confer some voting rights whereby the holder may vote in extraordinary general meetings. These are not the same as the ordinary voting rights conferred by ordinary shares.</skos:definition>
	</owl:ObjectProperty>
	
	<owl:DatatypeProperty rdf:about="&fibo-sec-eq-sha;numberOfSecurities">
		<rdfs:label xml:lang="en">number of securities</rdfs:label>
		<rdfs:domain rdf:resource="&fibo-sec-eq-sha;EquityConversionTerms"/>
		<rdfs:range rdf:resource="&xsd;integer"/>
		<skos:definition xml:lang="en">The number of units of the target security into which this security is converted upon conversion.</skos:definition>
	</owl:DatatypeProperty>
	
	<owl:ObjectProperty rdf:about="&fibo-sec-eq-sha;optionallyPays">
		<rdfs:label xml:lang="en">optionally pays</rdfs:label>
		<rdfs:domain rdf:resource="&fibo-sec-eq-sha;ParticipatingPreferenceShare"/>
		<rdfs:range rdf:resource="&fibo-md-eqx-pri;OrdinaryShareDividend"/>
	</owl:ObjectProperty>
	
	<owl:ObjectProperty rdf:about="&fibo-sec-eq-sha;participatingPreferenceShareSeniorToPreferenceShare">
		<rdfs:subPropertyOf rdf:resource="&fibo-sec-eq-sha;isSeniorToAClassOfPreferenceShare"/>
		<rdfs:label xml:lang="en">participating preference share senior to preference share</rdfs:label>
		<rdfs:domain rdf:resource="&fibo-sec-eq-sha;ParticipatingPreferenceShare"/>
		<rdfs:range rdf:resource="&fibo-sec-eq-sha;PreferenceShare"/>
	</owl:ObjectProperty>
	
	<owl:DatatypeProperty rdf:about="&fibo-sec-eq-sha;payInKind">
		<rdfs:label xml:lang="en">pay in kind</rdfs:label>
		<rdfs:domain rdf:resource="&fibo-sec-eq-sha;PreferredCouponPaymentTermSet"/>
		<rdfs:range rdf:resource="&xsd;boolean"/>
		<skos:definition xml:lang="en">The issuer will pay additional security as part of interest disbursement.</skos:definition>
	</owl:DatatypeProperty>
	
	<owl:ObjectProperty rdf:about="&fibo-sec-eq-sha;pays">
		<rdfs:label xml:lang="en">pays</rdfs:label>
		<rdfs:domain rdf:resource="&fibo-sec-eq-sha;OrdinaryShare"/>
		<rdfs:range rdf:resource="&fibo-md-eqx-pri;OrdinaryShareDividend"/>
	</owl:ObjectProperty>
	
	<owl:DatatypeProperty rdf:about="&fibo-sec-eq-sha;perpetual">
		<rdfs:label xml:lang="en">perpetual</rdfs:label>
		<rdfs:domain rdf:resource="&fibo-sec-eq-sha;PreferenceShare"/>
		<rdfs:range rdf:resource="&xsd;boolean"/>
		<skos:definition xml:lang="en">Signifies that there is NO set term involved. It pays its stated dividend forever or &quot;in perpetuity&quot;. For a fixed-rate a set dividend upon issue is agreed to, usually declared and paid quarterly (fixed dollar or a percent of the par value). For a floating-rate provide for a dividend that is paid by reference to a market interest rate.</skos:definition>
	</owl:DatatypeProperty>
	
	<owl:ObjectProperty rdf:about="&fibo-sec-eq-sha;preferenceShareSeniorToOrdinaryShare">
		<rdfs:subPropertyOf rdf:resource="&fibo-sec-eq-eq;isSeniorTo"/>
		<rdfs:label xml:lang="en">preference share senior to ordinary share</rdfs:label>
		<rdfs:domain rdf:resource="&fibo-sec-eq-sha;PreferenceShare"/>
		<rdfs:range rdf:resource="&fibo-sec-eq-sha;OrdinaryShare"/>
	</owl:ObjectProperty>
	
	<owl:ObjectProperty rdf:about="&fibo-sec-eq-sha;setsOut">
		<rdfs:label xml:lang="en">sets out</rdfs:label>
		<rdfs:domain rdf:resource="&fibo-be-oac-exec;ArticlesOfIncorporation"/>
		<rdfs:range rdf:resource="&fibo-sec-eq-sha;CompanyEquityTermsSet"/>
	</owl:ObjectProperty>
	
	<owl:DatatypeProperty rdf:about="&fibo-sec-eq-sha;softRetractable">
		<rdfs:label xml:lang="en">soft retractable</rdfs:label>
		<rdfs:domain rdf:resource="&fibo-sec-eq-sha;PreferenceShare"/>
		<rdfs:range rdf:resource="&xsd;boolean"/>
		<skos:definition xml:lang="en">A soft retraction value means it is payable in either &quot;hard cash&quot; or in an equal value of common stock of the issuer, at the choice of the issuer.</skos:definition>
	</owl:DatatypeProperty>

</rdf:RDF>