<?xml version="1.0" encoding="UTF-8"?>
<!DOCTYPE rdf:RDF [
	<!ENTITY dct "http://purl.org/dc/terms/">
	<!ENTITY fibo-be-oac-exec "https://spec.edmcouncil.org/fibo/ontology/BE/OwnershipAndControl/Executives/">
	<!ENTITY fibo-fnd-rel-rel "https://spec.edmcouncil.org/fibo/ontology/FND/Relations/Relations/">
	<!ENTITY fibo-fnd-utl-av "https://spec.edmcouncil.org/fibo/ontology/FND/Utilities/AnnotationVocabulary/">
	<!ENTITY fibo-sec-eq-eq "https://spec.edmcouncil.org/fibo/ontology/SEC/Equities/EquityInstruments/">
	<!ENTITY fibo-sec-eq-sha "https://spec.edmcouncil.org/fibo/ontology/SEC/Equities/ShareTerms/">
	<!ENTITY fibo-sec-eq-she "https://spec.edmcouncil.org/fibo/ontology/SEC/Equities/ShareholderEquity/">
	<!ENTITY owl "http://www.w3.org/2002/07/owl#">
	<!ENTITY rdf "http://www.w3.org/1999/02/22-rdf-syntax-ns#">
	<!ENTITY rdfs "http://www.w3.org/2000/01/rdf-schema#">
	<!ENTITY skos "http://www.w3.org/2004/02/skos/core#">
	<!ENTITY xsd "http://www.w3.org/2001/XMLSchema#">
]>
<rdf:RDF xml:base="https://spec.edmcouncil.org/fibo/ontology/SEC/Equities/ShareholderEquity/"
	xmlns:dct="http://purl.org/dc/terms/"
	xmlns:fibo-be-oac-exec="https://spec.edmcouncil.org/fibo/ontology/BE/OwnershipAndControl/Executives/"
	xmlns:fibo-fnd-rel-rel="https://spec.edmcouncil.org/fibo/ontology/FND/Relations/Relations/"
	xmlns:fibo-fnd-utl-av="https://spec.edmcouncil.org/fibo/ontology/FND/Utilities/AnnotationVocabulary/"
	xmlns:fibo-sec-eq-eq="https://spec.edmcouncil.org/fibo/ontology/SEC/Equities/EquityInstruments/"
	xmlns:fibo-sec-eq-sha="https://spec.edmcouncil.org/fibo/ontology/SEC/Equities/ShareTerms/"
	xmlns:fibo-sec-eq-she="https://spec.edmcouncil.org/fibo/ontology/SEC/Equities/ShareholderEquity/"
	xmlns:owl="http://www.w3.org/2002/07/owl#"
	xmlns:rdf="http://www.w3.org/1999/02/22-rdf-syntax-ns#"
	xmlns:rdfs="http://www.w3.org/2000/01/rdf-schema#"
	xmlns:skos="http://www.w3.org/2004/02/skos/core#"
	xmlns:xsd="http://www.w3.org/2001/XMLSchema#">
	
	<owl:Ontology rdf:about="https://spec.edmcouncil.org/fibo/ontology/SEC/Equities/ShareholderEquity/">
		<rdfs:label xml:lang="en">ShareholderEquity</rdfs:label>
		<dct:abstract>Shares are defined as instruments which confer equity on the holder. This ontology defines that equity and the various forms of equity that may be conferred on the holders of different share classes. These classes of equity have priority relationships between them so that for example senior equity has priority over more junior equity.</dct:abstract>
		<owl:imports rdf:resource="https://spec.edmcouncil.org/fibo/ontology/BE/OwnershipAndControl/Executives/"/>
		<owl:imports rdf:resource="https://spec.edmcouncil.org/fibo/ontology/FND/Relations/Relations/"/>
		<owl:imports rdf:resource="https://spec.edmcouncil.org/fibo/ontology/FND/Utilities/AnnotationVocabulary/"/>
		<owl:imports rdf:resource="https://spec.edmcouncil.org/fibo/ontology/SEC/Equities/EquityInstruments/"/>
		<owl:imports rdf:resource="https://spec.edmcouncil.org/fibo/ontology/SEC/Equities/ShareTerms/"/>
		<owl:versionIRI rdf:resource="https://spec.edmcouncil.org/fibo/ontology/SEC/Equities/ShareholderEquity/"/>
		<fibo-fnd-utl-av:hasMaturityLevel rdf:resource="&fibo-fnd-utl-av;Provisional"/>
	</owl:Ontology>
	
	<owl:Class rdf:about="&fibo-sec-eq-she;EquityPriorityTerms">
		<rdfs:subClassOf rdf:resource="&fibo-sec-eq-sha;CompanyEquityTermsSet"/>
		<rdfs:subClassOf>
			<owl:Restriction>
				<owl:onProperty rdf:resource="&fibo-sec-eq-she;confers"/>
				<owl:someValuesFrom rdf:resource="&fibo-sec-eq-she;ShareholderPrecedenceRight"/>
			</owl:Restriction>
		</rdfs:subClassOf>
		<rdfs:label xml:lang="en">equity priority terms</rdfs:label>
		<skos:definition xml:lang="en">Terms setting out the priority of a given class of Equity. These are the terms under which the holder of that class of equity has a call on the equity in the event of the issuing entity being wound up.</skos:definition>
		<fibo-fnd-utl-av:explanatoryNote xml:lang="en">this is one of the three kinds of term conferring three kinds of rights to the holder.</fibo-fnd-utl-av:explanatoryNote>
	</owl:Class>
	
	<owl:Class rdf:about="&fibo-sec-eq-she;JuniorEquity">
		<rdfs:subClassOf rdf:resource="&fibo-sec-eq-eq;ShareholderEquity"/>
		<rdfs:subClassOf>
			<owl:Restriction>
				<owl:onProperty rdf:resource="&fibo-sec-eq-she;hasPriorityAsDefinedIn"/>
				<owl:someValuesFrom rdf:resource="&fibo-sec-eq-she;JuniorEquityPriorityTermsSet"/>
			</owl:Restriction>
		</rdfs:subClassOf>
		<rdfs:label xml:lang="en">junior equity</rdfs:label>
		<skos:definition xml:lang="en">The most junior class of equity issued by a company. On the event of the company being wound up, holders of this class of equity have a call on the assets of the company only after the more senior classes of equity.</skos:definition>
	</owl:Class>
	
	<owl:Class rdf:about="&fibo-sec-eq-she;JuniorEquityPriorityTermsSet">
		<rdfs:subClassOf rdf:resource="&fibo-sec-eq-she;EquityPriorityTerms"/>
		<rdfs:label xml:lang="en">junior equity priority terms set</rdfs:label>
		<skos:definition xml:lang="en">The precise terms which define the seniority of this class of Equity. This is equity which has the lowest call on the assets of the issuer in the event of it being wound up, i.e. after Senior Equity and (if issued) other classes of equity.</skos:definition>
	</owl:Class>
	
	<owl:Class rdf:about="&fibo-sec-eq-she;OtherEquityPriorityTermsSet">
		<rdfs:subClassOf rdf:resource="&fibo-sec-eq-she;EquityPriorityTerms"/>
		<rdfs:label xml:lang="en">other equity priority terms set</rdfs:label>
		<skos:definition xml:lang="en">The precise terms which define the seniority of this class of Equity. These will set it apart from the highest of lowest seniority (senior or junior debt) and may be defined for more than one additional class of equity. These terms are defined by the issuer.</skos:definition>
	</owl:Class>
	
	<owl:Class rdf:about="&fibo-sec-eq-she;OtherSeniorityEquity">
		<rdfs:subClassOf rdf:resource="&fibo-sec-eq-eq;ShareholderEquity"/>
		<rdfs:subClassOf>
			<owl:Restriction>
				<owl:onProperty rdf:resource="&fibo-sec-eq-she;hasPriorityAsDefinedIn"/>
				<owl:someValuesFrom rdf:resource="&fibo-sec-eq-she;OtherEquityPriorityTermsSet"/>
			</owl:Restriction>
		</rdfs:subClassOf>
		<rdfs:label xml:lang="en">other seniority equity</rdfs:label>
		<skos:definition xml:lang="en">Equity which is neither the most senior nor the most junior. The precise terms under which this equity is held, and the definition of the call on the assets of the company in the event of it winding up, will be defined by the issuing company and are not modelled here as they may vary from one company to another. There may be more than one class of such equity issued by a company.</skos:definition>
	</owl:Class>
	
	<owl:Class rdf:about="&fibo-sec-eq-she;SeniorEquity">
		<rdfs:subClassOf rdf:resource="&fibo-sec-eq-eq;ShareholderEquity"/>
		<rdfs:subClassOf>
			<owl:Restriction>
				<owl:onProperty rdf:resource="&fibo-sec-eq-she;hasPriorityAsDefinedIn"/>
				<owl:someValuesFrom rdf:resource="&fibo-sec-eq-she;SeniorEquityPriorityTermsSet"/>
			</owl:Restriction>
		</rdfs:subClassOf>
		<rdfs:label xml:lang="en">senior equity</rdfs:label>
		<skos:definition xml:lang="en">The most senior class of equity issued in the company. Holders of this class of equity will receive first call on the assets of the company in the event of it being wound up.</skos:definition>
	</owl:Class>
	
	<owl:Class rdf:about="&fibo-sec-eq-she;SeniorEquityPriorityTermsSet">
		<rdfs:subClassOf rdf:resource="&fibo-sec-eq-she;EquityPriorityTerms"/>
		<rdfs:label xml:lang="en">senior equity priority terms set</rdfs:label>
		<skos:definition xml:lang="en">The precise terms which define the seniority of this class of Equity. These terms set out that the holder has the first call among equity holders, on the assets of the issuing entity in the event of it being wound up, ahead of the holders of other classes of equity.</skos:definition>
	</owl:Class>
	
	<owl:Class rdf:about="&fibo-sec-eq-she;ShareholderPrecedenceRight">
		<rdfs:subClassOf rdf:resource="&fibo-sec-eq-sha;PrecedenceRight"/>
		<rdfs:subClassOf>
			<owl:Restriction>
				<owl:onProperty rdf:resource="&fibo-fnd-rel-rel;isConferredBy"/>
				<owl:someValuesFrom rdf:resource="&fibo-be-oac-exec;ArticlesOfIncorporation"/>
			</owl:Restriction>
		</rdfs:subClassOf>
		<rdfs:label xml:lang="en">shareholder precedence right</rdfs:label>
		<skos:definition xml:lang="en">The rights of shareholderes in respect of the assets of the limited company in which they hold those shares, in the event of that company being wound up.</skos:definition>
		<fibo-fnd-utl-av:explanatoryNote xml:lang="en">These are defined, for different classes of equity, by the Company Articles of Association or equivalent Documentation. These are the rights defined in the Equity Priority Terms Set.</fibo-fnd-utl-av:explanatoryNote>
	</owl:Class>
	
	<owl:ObjectProperty rdf:about="&fibo-sec-eq-she;confers">
		<rdfs:label xml:lang="en">confers</rdfs:label>
		<rdfs:domain rdf:resource="&fibo-sec-eq-she;EquityPriorityTerms"/>
		<rdfs:range rdf:resource="&fibo-sec-eq-she;ShareholderPrecedenceRight"/>
	</owl:ObjectProperty>
	
	<owl:ObjectProperty rdf:about="&fibo-sec-eq-she;confersOwnershipOf">
		<rdfs:label>confers ownership of</rdfs:label>
	</owl:ObjectProperty>
	
	<owl:ObjectProperty rdf:about="&fibo-sec-eq-she;confersOwnershipOf.1">
		<rdfs:label>confers ownership of</rdfs:label>
	</owl:ObjectProperty>
	
	<owl:ObjectProperty rdf:about="&fibo-sec-eq-she;hasPriorityAsDefinedIn">
		<rdfs:label xml:lang="en">has priority as defined in</rdfs:label>
		<rdfs:domain rdf:resource="&fibo-sec-eq-eq;ShareholderEquity"/>
		<rdfs:range rdf:resource="&fibo-sec-eq-she;EquityPriorityTerms"/>
	</owl:ObjectProperty>
	
	<owl:ObjectProperty rdf:about="&fibo-sec-eq-she;juniorEquityPriority">
		<rdfs:subPropertyOf rdf:resource="&fibo-sec-eq-eq;priority"/>
		<rdfs:label xml:lang="en">junior equity priority</rdfs:label>
		<rdfs:domain rdf:resource="&fibo-sec-eq-she;JuniorEquity"/>
		<rdfs:range rdf:resource="&fibo-sec-eq-eq;Junior"/>
		<skos:definition xml:lang="en">The seniority of the equity. This is the order of precedence in which holders of different classes of equity will have a call on the assets of the company in the event of it winding up. In the case of ordinary equity this is the lowest seniority i.e. it has the last call on the assets of the company.</skos:definition>
	</owl:ObjectProperty>
	
	<owl:ObjectProperty rdf:about="&fibo-sec-eq-she;otherEquityPriority">
		<rdfs:subPropertyOf rdf:resource="&fibo-sec-eq-eq;priority"/>
		<rdfs:label xml:lang="en">other equity priority</rdfs:label>
		<rdfs:domain rdf:resource="&fibo-sec-eq-she;OtherSeniorityEquity"/>
		<rdfs:range rdf:resource="&fibo-sec-eq-eq;OtherSeniority"/>
		<skos:definition xml:lang="en">The seniority of the equity. This is the order of precedence in which holders of different classes of equity will have a call on the assets of the company in the event of it winding up. In this class of equity this is defined as being &quot;Other&quot; than highest or lowest, with the precise terms and order of precedence being defined in the priority terms.</skos:definition>
	</owl:ObjectProperty>
	
	<owl:ObjectProperty rdf:about="&fibo-sec-eq-she;seniorEquityPriority">
		<rdfs:subPropertyOf rdf:resource="&fibo-sec-eq-eq;priority"/>
		<rdfs:label xml:lang="en">senior equity priority</rdfs:label>
		<rdfs:domain rdf:resource="&fibo-sec-eq-she;SeniorEquity"/>
		<rdfs:range rdf:resource="&fibo-sec-eq-eq;Senior"/>
		<skos:definition xml:lang="en">The seniority of the equity. This is the order of precedence in which holders of different classes of equity will have a call on the assets of the company in the event of it winding up. In this class of equity this is the highest in senioity.</skos:definition>
	</owl:ObjectProperty>

</rdf:RDF>