<?xml version="1.0" encoding="UTF-8"?>
<!DOCTYPE rdf:RDF [
	<!ENTITY dct "http://purl.org/dc/terms/">
	<!ENTITY fibo-fbc-fi-fi "https://spec.edmcouncil.org/fibo/ontology/FBC/FinancialInstruments/FinancialInstruments/">
	<!ENTITY fibo-fnd-acc-aeq "https://spec.edmcouncil.org/fibo/ontology/FND/Accounting/AccountingEquity/">
	<!ENTITY fibo-fnd-acc-cur "https://spec.edmcouncil.org/fibo/ontology/FND/Accounting/CurrencyAmount/">
	<!ENTITY fibo-fnd-agr-agr "https://spec.edmcouncil.org/fibo/ontology/FND/Agreements/Agreements/">
	<!ENTITY fibo-fnd-agr-ctr "https://spec.edmcouncil.org/fibo/ontology/FND/Agreements/Contracts/">
	<!ENTITY fibo-fnd-dt-bd "https://spec.edmcouncil.org/fibo/ontology/FND/DatesAndTimes/BusinessDates/">
	<!ENTITY fibo-fnd-dt-fd "https://spec.edmcouncil.org/fibo/ontology/FND/DatesAndTimes/FinancialDates/">
	<!ENTITY fibo-fnd-law-lcap "https://spec.edmcouncil.org/fibo/ontology/FND/Law/LegalCapacity/">
	<!ENTITY fibo-fnd-pas-psch "https://spec.edmcouncil.org/fibo/ontology/FND/ProductsAndServices/PaymentsAndSchedules/">
	<!ENTITY fibo-fnd-rel-rel "https://spec.edmcouncil.org/fibo/ontology/FND/Relations/Relations/">
	<!ENTITY fibo-fnd-utl-av "https://spec.edmcouncil.org/fibo/ontology/FND/Utilities/AnnotationVocabulary/">
	<!ENTITY fibo-sec-eq-eq "https://spec.edmcouncil.org/fibo/ontology/SEC/Equities/EquityInstruments/">
	<!ENTITY fibo-sec-eq-mod "https://spec.edmcouncil.org/fibo/ontology/SEC/Equities/MetadataSECEquities/">
	<!ENTITY fibo-sec-eq-sha "https://spec.edmcouncil.org/fibo/ontology/SEC/Equities/ShareTerms/">
	<!ENTITY fibo-sec-sec-iss "https://spec.edmcouncil.org/fibo/ontology/SEC/Securities/SecuritiesIssuance/">
	<!ENTITY fibo-sec-sec-lst "https://spec.edmcouncil.org/fibo/ontology/SEC/Securities/SecuritiesListings/">
	<!ENTITY owl "http://www.w3.org/2002/07/owl#">
	<!ENTITY rdf "http://www.w3.org/1999/02/22-rdf-syntax-ns#">
	<!ENTITY rdfs "http://www.w3.org/2000/01/rdf-schema#">
	<!ENTITY skos "http://www.w3.org/2004/02/skos/core#">
	<!ENTITY sm "http://www.omg.org/techprocess/ab/SpecificationMetadata/">
	<!ENTITY xsd "http://www.w3.org/2001/XMLSchema#">
]>
<rdf:RDF xml:base="https://spec.edmcouncil.org/fibo/ontology/SEC/Equities/ShareTerms/"
	xmlns:dct="http://purl.org/dc/terms/"
	xmlns:fibo-fbc-fi-fi="https://spec.edmcouncil.org/fibo/ontology/FBC/FinancialInstruments/FinancialInstruments/"
	xmlns:fibo-fnd-acc-aeq="https://spec.edmcouncil.org/fibo/ontology/FND/Accounting/AccountingEquity/"
	xmlns:fibo-fnd-acc-cur="https://spec.edmcouncil.org/fibo/ontology/FND/Accounting/CurrencyAmount/"
	xmlns:fibo-fnd-agr-agr="https://spec.edmcouncil.org/fibo/ontology/FND/Agreements/Agreements/"
	xmlns:fibo-fnd-agr-ctr="https://spec.edmcouncil.org/fibo/ontology/FND/Agreements/Contracts/"
	xmlns:fibo-fnd-dt-bd="https://spec.edmcouncil.org/fibo/ontology/FND/DatesAndTimes/BusinessDates/"
	xmlns:fibo-fnd-dt-fd="https://spec.edmcouncil.org/fibo/ontology/FND/DatesAndTimes/FinancialDates/"
	xmlns:fibo-fnd-law-lcap="https://spec.edmcouncil.org/fibo/ontology/FND/Law/LegalCapacity/"
	xmlns:fibo-fnd-pas-psch="https://spec.edmcouncil.org/fibo/ontology/FND/ProductsAndServices/PaymentsAndSchedules/"
	xmlns:fibo-fnd-rel-rel="https://spec.edmcouncil.org/fibo/ontology/FND/Relations/Relations/"
	xmlns:fibo-fnd-utl-av="https://spec.edmcouncil.org/fibo/ontology/FND/Utilities/AnnotationVocabulary/"
	xmlns:fibo-sec-eq-eq="https://spec.edmcouncil.org/fibo/ontology/SEC/Equities/EquityInstruments/"
	xmlns:fibo-sec-eq-mod="https://spec.edmcouncil.org/fibo/ontology/SEC/Equities/MetadataSECEquities/"
	xmlns:fibo-sec-eq-sha="https://spec.edmcouncil.org/fibo/ontology/SEC/Equities/ShareTerms/"
	xmlns:fibo-sec-sec-iss="https://spec.edmcouncil.org/fibo/ontology/SEC/Securities/SecuritiesIssuance/"
	xmlns:fibo-sec-sec-lst="https://spec.edmcouncil.org/fibo/ontology/SEC/Securities/SecuritiesListings/"
	xmlns:owl="http://www.w3.org/2002/07/owl#"
	xmlns:rdf="http://www.w3.org/1999/02/22-rdf-syntax-ns#"
	xmlns:rdfs="http://www.w3.org/2000/01/rdf-schema#"
	xmlns:skos="http://www.w3.org/2004/02/skos/core#"
	xmlns:sm="http://www.omg.org/techprocess/ab/SpecificationMetadata/"
	xmlns:xsd="http://www.w3.org/2001/XMLSchema#">
	
	<owl:Ontology rdf:about="https://spec.edmcouncil.org/fibo/ontology/SEC/Equities/ShareTerms/">
		<rdfs:label>Share Terms Ontology</rdfs:label>
		<dct:abstract>This ontology defines the kinds of terms that different clases of share may have, and that distinguish these from one another. These includes different combinations of voting rights, dividend terms, share coupons, participating and precedence terms as well as terms for convertible shares. This ontology also defines classes of share that are defined by differences in these rights and precedences, and the class of convertible shares.</dct:abstract>
		<dct:isPartOf rdf:resource="&fibo-sec-eq-mod;EquitiesModule"/>
		<dct:license rdf:datatype="&xsd;anyURI">http://opensource.org/licenses/MIT</dct:license>
		<sm:contentLanguage rdf:datatype="&xsd;anyURI">http://www.w3.org/standards/techs/owl#w3c_all</sm:contentLanguage>
		<sm:copyright>Copyright (c) 2013-2018 EDM Council, Inc.</sm:copyright>
		<sm:fileAbbreviation>fibo-sec-eq-sha</sm:fileAbbreviation>
		<sm:filename>ShareTerms.rdf</sm:filename>
		<owl:imports rdf:resource="https://spec.edmcouncil.org/fibo/ontology/FBC/FinancialInstruments/FinancialInstruments/"/>
		<owl:imports rdf:resource="https://spec.edmcouncil.org/fibo/ontology/FND/Accounting/AccountingEquity/"/>
		<owl:imports rdf:resource="https://spec.edmcouncil.org/fibo/ontology/FND/Accounting/CurrencyAmount/"/>
		<owl:imports rdf:resource="https://spec.edmcouncil.org/fibo/ontology/FND/Agreements/Agreements/"/>
		<owl:imports rdf:resource="https://spec.edmcouncil.org/fibo/ontology/FND/Agreements/Contracts/"/>
		<owl:imports rdf:resource="https://spec.edmcouncil.org/fibo/ontology/FND/DatesAndTimes/BusinessDates/"/>
		<owl:imports rdf:resource="https://spec.edmcouncil.org/fibo/ontology/FND/DatesAndTimes/FinancialDates/"/>
		<owl:imports rdf:resource="https://spec.edmcouncil.org/fibo/ontology/FND/Law/LegalCapacity/"/>
		<owl:imports rdf:resource="https://spec.edmcouncil.org/fibo/ontology/FND/ProductsAndServices/PaymentsAndSchedules/"/>
		<owl:imports rdf:resource="https://spec.edmcouncil.org/fibo/ontology/FND/Relations/Relations/"/>
		<owl:imports rdf:resource="https://spec.edmcouncil.org/fibo/ontology/FND/Utilities/AnnotationVocabulary/"/>
		<owl:imports rdf:resource="https://spec.edmcouncil.org/fibo/ontology/SEC/Equities/EquityInstruments/"/>
		<owl:imports rdf:resource="https://spec.edmcouncil.org/fibo/ontology/SEC/Equities/MetadataSECEquities/"/>
		<owl:imports rdf:resource="https://spec.edmcouncil.org/fibo/ontology/SEC/Securities/SecuritiesIssuance/"/>
		<owl:imports rdf:resource="https://spec.edmcouncil.org/fibo/ontology/SEC/Securities/SecuritiesListings/"/>
		<owl:versionIRI rdf:resource="https://spec.edmcouncil.org/fibo/ontology/SEC/Equities/ShareTerms/"/>
		<fibo-fnd-utl-av:hasMaturityLevel rdf:resource="&fibo-fnd-utl-av;Provisional"/>
	</owl:Ontology>
	
	<owl:Class rdf:about="&fibo-sec-eq-eq;CommonShare">
		<rdfs:subClassOf>
			<owl:Restriction>
				<owl:onProperty rdf:resource="&fibo-sec-eq-sha;pays"/>
				<owl:minQualifiedCardinality rdf:datatype="&xsd;nonNegativeInteger">0</owl:minQualifiedCardinality>
				<owl:someValuesFrom rdf:resource="&fibo-sec-eq-sha;OrdinaryDividend"/>
			</owl:Restriction>
		</rdfs:subClassOf>
		<owl:disjointWith rdf:resource="&fibo-sec-eq-sha;PreferredShare"/>
	</owl:Class>
	
	<owl:Class rdf:about="&fibo-sec-eq-sha;ConvertiblePreferredShare">
		<rdfs:subClassOf rdf:resource="&fibo-sec-eq-sha;PreferredShare"/>
		<rdfs:subClassOf rdf:resource="&fibo-sec-sec-iss;ConvertibleSecurity"/>
		<rdfs:subClassOf>
			<owl:Restriction>
				<owl:onProperty rdf:resource="&fibo-fnd-agr-ctr;hasContractualElement"/>
				<owl:someValuesFrom rdf:resource="&fibo-sec-eq-sha;EquityConversionTerms"/>
			</owl:Restriction>
		</rdfs:subClassOf>
		<rdfs:label>convertible preferred share</rdfs:label>
		<skos:definition>a preferred share that is convertible into another security</skos:definition>
	</owl:Class>
	
	<owl:Class rdf:about="&fibo-sec-eq-sha;CumulativePreferredShare">
		<rdfs:subClassOf rdf:resource="&fibo-sec-eq-sha;PreferredShare"/>
		<rdfs:label>cumulative preferred share</rdfs:label>
		<skos:definition>a preferred share whose dividends, if not paid due to insufficient earnings or other reasons, accumulate until paid out</skos:definition>
		<fibo-fnd-utl-av:explanatoryNote>These dividends have precedence over ordinary dividends which cannot be paid until any cumulative dividend obligations have been paid.</fibo-fnd-utl-av:explanatoryNote>
	</owl:Class>
	
	<owl:NamedIndividual rdf:about="&fibo-sec-eq-sha;DistributionByCashPayment">
		<rdf:type rdf:resource="&fibo-sec-eq-sha;DividendDistributionMethod"/>
		<rdfs:label>distribution by payment</rdfs:label>
		<skos:definition>a distribution method involving payment of cash to the shareholder</skos:definition>
	</owl:NamedIndividual>
	
	<owl:NamedIndividual rdf:about="&fibo-sec-eq-sha;DistributionByReinvestment">
		<rdf:type rdf:resource="&fibo-sec-eq-sha;DividendDistributionMethod"/>
		<rdfs:label>distribution by reinvestment</rdfs:label>
		<skos:definition>a distribution method involving automatic reinvestment of shareholders&apos; dividends in additional, potentially fractional, shares in the same equity or fund</skos:definition>
	</owl:NamedIndividual>
	
	<owl:Class rdf:about="&fibo-sec-eq-sha;Dividend">
		<rdfs:subClassOf rdf:resource="&fibo-fnd-agr-agr;Commitment"/>
		<rdfs:subClassOf>
			<owl:Restriction>
				<owl:onProperty rdf:resource="&fibo-fnd-pas-psch;hasPaymentAmount"/>
				<owl:onClass rdf:resource="&fibo-fnd-acc-cur;MonetaryAmount"/>
				<owl:maxQualifiedCardinality rdf:datatype="&xsd;nonNegativeInteger">1</owl:maxQualifiedCardinality>
			</owl:Restriction>
		</rdfs:subClassOf>
		<rdfs:subClassOf>
			<owl:Restriction>
				<owl:onProperty rdf:resource="&fibo-sec-eq-sha;hasDistributionMethod"/>
				<owl:onClass rdf:resource="&fibo-sec-eq-sha;DividendDistributionMethod"/>
				<owl:maxQualifiedCardinality rdf:datatype="&xsd;nonNegativeInteger">1</owl:maxQualifiedCardinality>
			</owl:Restriction>
		</rdfs:subClassOf>
		<rdfs:subClassOf>
			<owl:Restriction>
				<owl:onProperty rdf:resource="&fibo-fnd-dt-fd;hasSchedule"/>
				<owl:onClass rdf:resource="&fibo-sec-eq-sha;DividendOrShareCouponSchedule"/>
				<owl:maxQualifiedCardinality rdf:datatype="&xsd;nonNegativeInteger">1</owl:maxQualifiedCardinality>
			</owl:Restriction>
		</rdfs:subClassOf>
		<rdfs:label>dividend</rdfs:label>
		<skos:definition>a commitment to distribute a portion of earnings to shareholders, prorated by class of security, to be paid in the form of money, shares, scrip, or on rare occasion, property</skos:definition>
		<fibo-fnd-utl-av:explanatoryNote>The amount and timing of payment is set by the board of directors, typically quarterly.</fibo-fnd-utl-av:explanatoryNote>
	</owl:Class>
	
	<owl:Class rdf:about="&fibo-sec-eq-sha;DividendDistributionMethod">
		<rdfs:subClassOf rdf:resource="&fibo-fnd-dt-bd;Convention"/>
		<rdfs:label>dividend distribution method</rdfs:label>
		<skos:definition>the convention by which dividends are distributed, i.e., by payment of a monetary amount or by reinvestment, as specified by the board of directors at the time a decision to issue a dividend is made</skos:definition>
	</owl:Class>
	
	<owl:Class rdf:about="&fibo-sec-eq-sha;DividendOrShareCouponSchedule">
		<rdfs:subClassOf rdf:resource="&fibo-fnd-dt-fd;RegularSchedule"/>
		<rdfs:subClassOf rdf:resource="&fibo-fnd-pas-psch;PaymentSchedule"/>
		<rdfs:label>dividend or share coupon schedule</rdfs:label>
		<skos:definition>a payment schedule indicating the dates on which dividends or share coupon payments are due to be paid</skos:definition>
	</owl:Class>
	
	<owl:Class rdf:about="&fibo-sec-eq-sha;EquityConversionTerms">
		<rdfs:subClassOf rdf:resource="&fibo-sec-sec-iss;ConversionTerms"/>
		<rdfs:subClassOf>
			<owl:Restriction>
				<owl:onProperty rdf:resource="&fibo-sec-eq-sha;specifiesConversionDate"/>
				<owl:someValuesFrom rdf:resource="&fibo-fnd-dt-fd;Date"/>
			</owl:Restriction>
		</rdfs:subClassOf>
		<rdfs:subClassOf>
			<owl:Restriction>
				<owl:onProperty rdf:resource="&fibo-sec-sec-iss;specifiesConversionInto"/>
				<owl:someValuesFrom rdf:resource="&fibo-fbc-fi-fi;Security"/>
			</owl:Restriction>
		</rdfs:subClassOf>
		<rdfs:label>equity conversion terms</rdfs:label>
		<skos:definition>conversion terms specifying the details regarding conversion of shares into other securities</skos:definition>
	</owl:Class>
	
	<owl:Class rdf:about="&fibo-sec-eq-sha;ExtraordinaryVotingRight">
		<rdfs:subClassOf rdf:resource="&fibo-sec-eq-eq;VotingRight"/>
		<rdfs:label>extraordinary voting right</rdfs:label>
		<skos:definition>the right to vote at extraordinary meetings, as opposed to being able to vote strictly at annual general meetings</skos:definition>
	</owl:Class>
	
	<owl:Class rdf:about="&fibo-sec-eq-sha;NonCumulativePreferredShare">
		<rdfs:subClassOf rdf:resource="&fibo-sec-eq-sha;PreferredShare"/>
		<rdfs:label>non-cumulative preferred share</rdfs:label>
		<owl:disjointWith rdf:resource="&fibo-sec-eq-sha;CumulativePreferredShare"/>
		<skos:definition>a preferred share whose dividend payments are not carried forward</skos:definition>
	</owl:Class>
	
	<owl:Class rdf:about="&fibo-sec-eq-sha;NonParticipatingPreferredShare">
		<rdfs:subClassOf rdf:resource="&fibo-sec-eq-sha;PreferredShare"/>
		<rdfs:label>non-participating preferred share</rdfs:label>
		<owl:disjointWith rdf:resource="&fibo-sec-eq-sha;ParticipatingPreferredShare"/>
		<skos:definition>a preferred share that is not a participating preferred share</skos:definition>
	</owl:Class>
	
	<owl:Class rdf:about="&fibo-sec-eq-sha;OrdinaryDividend">
		<rdfs:subClassOf rdf:resource="&fibo-sec-eq-sha;Dividend"/>
		<rdfs:label>ordinary dividend</rdfs:label>
		<skos:definition>a dividend that is taxed as ordinary income on receipt by a shareholder</skos:definition>
		<fibo-fnd-utl-av:explanatoryNote>Most dividends are considered ordinary, unless they are specifically designated as qualified dividends.</fibo-fnd-utl-av:explanatoryNote>
		<fibo-fnd-utl-av:explanatoryNote>Note that the terms related to ordinary dividend payment are typically specified in the context of a board resolution rather than contractually.</fibo-fnd-utl-av:explanatoryNote>
	</owl:Class>
	
	<owl:Class rdf:about="&fibo-sec-eq-sha;OrdinaryVotingRight">
		<rdfs:subClassOf rdf:resource="&fibo-sec-eq-eq;VotingRight"/>
		<rdfs:label>ordinary voting right</rdfs:label>
		<skos:definition>voting right conferred on holders of common shares, as defined by the issuer</skos:definition>
	</owl:Class>
	
	<owl:Class rdf:about="&fibo-sec-eq-sha;ParticipatingPreferredShare">
		<rdfs:subClassOf rdf:resource="&fibo-sec-eq-sha;PreferredShare"/>
		<rdfs:subClassOf>
			<owl:Restriction>
				<owl:onProperty rdf:resource="&fibo-sec-eq-sha;pays"/>
				<owl:onClass rdf:resource="&fibo-sec-eq-sha;OrdinaryDividend"/>
				<owl:minQualifiedCardinality rdf:datatype="&xsd;nonNegativeInteger">0</owl:minQualifiedCardinality>
			</owl:Restriction>
		</rdfs:subClassOf>
		<rdfs:label>participating preferred share</rdfs:label>
		<skos:definition>a preferred share that, in addition to paying a stipulated dividend, gives the holder the right to participate with common share holders in additional distributions of earnings under specified conditions</skos:definition>
		<fibo-fnd-utl-av:explanatoryNote>Participating preferred shares are rare, typically only issued when needed to attract investors.</fibo-fnd-utl-av:explanatoryNote>
	</owl:Class>
	
	<owl:Class rdf:about="&fibo-sec-eq-sha;PrecedenceRight">
		<rdfs:subClassOf rdf:resource="&fibo-fnd-law-lcap;ContractualRight"/>
		<rdfs:label>precedence right</rdfs:label>
		<skos:definition>the rights of various parties in respect of the assets of some entity in the event of that entity being wound up</skos:definition>
		<fibo-fnd-utl-av:explanatoryNote>Some of these rights are enshrined in law. A special case of these is shareholder rights which are defined, for different classes of equity, by the Company Articles of Association or equivalent Documentation. These are the rights defined in the Equity Priority Terms Set.</fibo-fnd-utl-av:explanatoryNote>
	</owl:Class>
	
	<owl:Class rdf:about="&fibo-sec-eq-sha;PreferredShare">
		<rdfs:subClassOf rdf:resource="&fibo-sec-eq-eq;Share"/>
		<rdfs:subClassOf>
			<owl:Restriction>
				<owl:onProperty rdf:resource="&fibo-fnd-rel-rel;confers"/>
				<owl:onClass rdf:resource="&fibo-sec-eq-sha;ExtraordinaryVotingRight"/>
				<owl:minQualifiedCardinality rdf:datatype="&xsd;nonNegativeInteger">0</owl:minQualifiedCardinality>
			</owl:Restriction>
		</rdfs:subClassOf>
		<rdfs:subClassOf>
			<owl:Restriction>
				<owl:onProperty rdf:resource="&fibo-sec-eq-sha;hasCoupon"/>
				<owl:someValuesFrom>
					<owl:Class>
						<owl:unionOf rdf:parseType="Collection">
							<rdf:Description rdf:about="&fibo-sec-eq-sha;OrdinaryDividend">
							</rdf:Description>
							<rdf:Description rdf:about="&fibo-sec-eq-sha;PreferredShareCoupon">
							</rdf:Description>
						</owl:unionOf>
					</owl:Class>
				</owl:someValuesFrom>
			</owl:Restriction>
		</rdfs:subClassOf>
		<rdfs:subClassOf>
			<owl:Restriction>
				<owl:onProperty rdf:resource="&fibo-sec-eq-sha;isSeniorTo"/>
				<owl:someValuesFrom rdf:resource="&fibo-sec-eq-eq;CommonShare"/>
			</owl:Restriction>
		</rdfs:subClassOf>
		<rdfs:label>preferred share</rdfs:label>
		<skos:definition>a share that pays dividends at a specified rate and has preference over common shares in the payment of dividends and liquidation of corporate assets</skos:definition>
	</owl:Class>
	
	<owl:Class rdf:about="&fibo-sec-eq-sha;PreferredShareCoupon">
		<rdfs:subClassOf rdf:resource="&fibo-fnd-agr-agr;Commitment"/>
		<rdfs:subClassOf>
			<owl:Restriction>
				<owl:onProperty rdf:resource="&fibo-fnd-pas-psch;hasPaymentAmount"/>
				<owl:onClass rdf:resource="&fibo-fnd-acc-cur;MonetaryAmount"/>
				<owl:maxQualifiedCardinality rdf:datatype="&xsd;nonNegativeInteger">1</owl:maxQualifiedCardinality>
			</owl:Restriction>
		</rdfs:subClassOf>
		<rdfs:subClassOf>
			<owl:Restriction>
				<owl:onProperty rdf:resource="&fibo-sec-eq-sha;hasDividendRate"/>
				<owl:onClass rdf:resource="&fibo-fnd-acc-cur;PercentageMonetaryAmount"/>
				<owl:maxQualifiedCardinality rdf:datatype="&xsd;nonNegativeInteger">1</owl:maxQualifiedCardinality>
			</owl:Restriction>
		</rdfs:subClassOf>
		<rdfs:subClassOf>
			<owl:Restriction>
				<owl:onProperty rdf:resource="&fibo-sec-eq-sha;hasGracePeriod"/>
				<owl:onClass rdf:resource="&fibo-fnd-dt-fd;Duration"/>
				<owl:maxQualifiedCardinality rdf:datatype="&xsd;nonNegativeInteger">1</owl:maxQualifiedCardinality>
			</owl:Restriction>
		</rdfs:subClassOf>
		<rdfs:subClassOf>
			<owl:Restriction>
				<owl:onProperty rdf:resource="&fibo-sec-eq-sha;hasDistributionMethod"/>
				<owl:onClass rdf:resource="&fibo-sec-eq-sha;DividendDistributionMethod"/>
				<owl:maxQualifiedCardinality rdf:datatype="&xsd;nonNegativeInteger">1</owl:maxQualifiedCardinality>
			</owl:Restriction>
		</rdfs:subClassOf>
		<rdfs:subClassOf>
			<owl:Restriction>
				<owl:onProperty rdf:resource="&fibo-fnd-dt-fd;hasSchedule"/>
				<owl:onClass rdf:resource="&fibo-sec-eq-sha;DividendOrShareCouponSchedule"/>
				<owl:maxQualifiedCardinality rdf:datatype="&xsd;nonNegativeInteger">1</owl:maxQualifiedCardinality>
			</owl:Restriction>
		</rdfs:subClassOf>
		<rdfs:label>preferred share coupon</rdfs:label>
		<skos:definition>a commitment to distribute a portion of earnings to shareholders, similar to a dividend but often with a fixed payment amount and schedule</skos:definition>
	</owl:Class>
	
	<owl:Class rdf:about="&fibo-sec-eq-sha;QualifiedDividend">
		<rdfs:subClassOf rdf:resource="&fibo-sec-eq-sha;Dividend"/>
		<rdfs:label>qualified dividend</rdfs:label>
		<skos:definition>a dividend that falls under capital gains tax rates that are lower than the income tax rates on unqualified, or ordinary, dividends</skos:definition>
	</owl:Class>
	
	<owl:Class rdf:about="&fibo-sec-eq-sha;RestrictedVotingRight">
		<rdfs:subClassOf rdf:resource="&fibo-sec-eq-eq;VotingRight"/>
		<rdfs:label>restricted voting right</rdfs:label>
		<skos:definition>a voting right that has certain limitations associated with it</skos:definition>
	</owl:Class>
	
	<owl:ObjectProperty rdf:about="&fibo-sec-eq-sha;hasCoupon">
		<rdfs:subPropertyOf rdf:resource="&fibo-fnd-rel-rel;has"/>
		<rdfs:label>has coupon</rdfs:label>
		<rdfs:domain rdf:resource="&fibo-sec-eq-sha;PreferredShare"/>
		<rdfs:range>
			<owl:Class>
				<owl:unionOf rdf:parseType="Collection">
					<rdf:Description rdf:about="&fibo-sec-eq-sha;OrdinaryDividend">
					</rdf:Description>
					<rdf:Description rdf:about="&fibo-sec-eq-sha;PreferredShareCoupon">
					</rdf:Description>
				</owl:unionOf>
			</owl:Class>
		</rdfs:range>
		<skos:definition>relates a preferred share to a dividend or coupon that applies to the share</skos:definition>
	</owl:ObjectProperty>
	
	<owl:ObjectProperty rdf:about="&fibo-sec-eq-sha;hasDistributionMethod">
		<rdfs:subPropertyOf rdf:resource="&fibo-fnd-rel-rel;has"/>
		<rdfs:label>has distribution method</rdfs:label>
		<rdfs:domain rdf:resource="&fibo-sec-eq-sha;Dividend"/>
		<rdfs:range rdf:resource="&fibo-sec-eq-sha;DividendDistributionMethod"/>
		<skos:definition>indicates the method by which dividend or coupon payments are to be distributed</skos:definition>
	</owl:ObjectProperty>
	
	<owl:ObjectProperty rdf:about="&fibo-sec-eq-sha;hasDividendRate">
		<rdfs:subPropertyOf rdf:resource="&fibo-fnd-rel-rel;has"/>
		<rdfs:label>has dividend rate</rdfs:label>
		<rdfs:domain rdf:resource="&fibo-sec-eq-sha;PreferredShareCoupon"/>
		<rdfs:range rdf:resource="&fibo-fnd-acc-cur;PercentageMonetaryAmount"/>
		<skos:definition>indicates a pre-arranged dividend rate</skos:definition>
	</owl:ObjectProperty>
	
	<owl:ObjectProperty rdf:about="&fibo-sec-eq-sha;hasGracePeriod">
		<rdfs:subPropertyOf rdf:resource="&fibo-fnd-dt-fd;hasDuration"/>
		<rdfs:label>has grace period</rdfs:label>
		<rdfs:domain rdf:resource="&fibo-sec-eq-sha;PreferredShareCoupon"/>
		<rdfs:range rdf:resource="&fibo-fnd-dt-fd;Duration"/>
		<skos:definition>indicates a period of time after a coupon payment becomes due, before the issuer is subject to penalties</skos:definition>
	</owl:ObjectProperty>
	
	<owl:ObjectProperty rdf:about="&fibo-sec-eq-sha;isSeniorTo">
		<rdfs:label>is senior to</rdfs:label>
		<rdfs:domain rdf:resource="&fibo-sec-eq-eq;Share"/>
		<rdfs:range rdf:resource="&fibo-sec-eq-eq;Share"/>
		<skos:definition>indicates that a given share (share class) has higher seniority than the related share, meaning that it gives the holder a higher claim on the assets of the issuer</skos:definition>
	</owl:ObjectProperty>
	
	<owl:ObjectProperty rdf:about="&fibo-sec-eq-sha;pays">
		<rdfs:label>pays</rdfs:label>
		<rdfs:domain rdf:resource="&fibo-sec-eq-eq;Share"/>
		<rdfs:range rdf:resource="&fibo-sec-eq-sha;Dividend"/>
		<skos:definition>relates a share to a dividend that it may pay to shareholders</skos:definition>
	</owl:ObjectProperty>
	
	<owl:ObjectProperty rdf:about="&fibo-sec-eq-sha;specifiesConversionDate">
		<rdfs:label>specifies conversion date</rdfs:label>
		<rdfs:domain rdf:resource="&fibo-sec-eq-sha;EquityConversionTerms"/>
		<rdfs:range rdf:resource="&fibo-fnd-dt-fd;Date"/>
		<skos:definition>indicates the date on which, or after which, conversion may occur</skos:definition>
	</owl:ObjectProperty>

</rdf:RDF>