<?xml version="1.0" encoding="UTF-8"?>
<rdf:RDF xmlns:xsd="http://www.w3.org/2001/XMLSchema#"
         xmlns:sm="http://www.omg.org/techprocess/ab/SpecificationMetadata/"
         xmlns:fibo-fnd-utl-av="http://www.omg.org/spec/EDMC-FIBO/FND/Utilities/AnnotationVocabulary/"
         xmlns:rdf="http://www.w3.org/1999/02/22-rdf-syntax-ns#"
         xmlns:rdfs="http://www.w3.org/2000/01/rdf-schema#"
         xmlns:owl="http://www.w3.org/2002/07/owl#"
         xmlns:skos="http://www.w3.org/2004/02/skos/core#"
         xmlns:dc="http://purl.org/dc/terms/"
         xml:base="http://www.edmcouncil.org/spec/EDMC-SR/FND/Relative/ToolsAndInstruments/">

   <owl:Ontology rdf:about="http://www.edmcouncil.org/spec/EDMC-SR/FND/Relative/ToolsAndInstruments/">
      <owl:imports rdf:resource="http://www.edmcouncil.org/spec/EDMC-SR/UO/OntologicalDegree/"/>
      <owl:imports rdf:resource="http://www.edmcouncil.org/spec/EDMC-SR/UO/Lattice/"/>
   </owl:Ontology>

   <!--Datatypes-->

<!--Object Properties-->

<owl:ObjectProperty rdf:about="http://www.edmcouncil.org/spec/EDMC-SR/FND/Relative/ToolsAndInstruments/measurementInstrumentHasPurpose">
      <skos:definition>The purpose to which some measurement instrument is put, is to measure something. Scope Note: not in scope for financial services, this is just here to illustrate the context of the surrounding terms.</skos:definition>
      <rdfs:subPropertyOf rdf:resource="http://www.edmcouncil.org/spec/EDMC-SR/FND/Relative/ToolsAndInstruments/hasPurpose"/>
      <rdfs:domain rdf:resource="http://www.edmcouncil.org/spec/EDMC-SR/FND/Relative/ToolsAndInstruments/MeasurementInstrument"/>
      <rdfs:range rdf:resource="http://www.edmcouncil.org/spec/EDMC-SR/FND/Relative/ToolsAndInstruments/MeasurementPurpose"/>
   </owl:ObjectProperty>

   <owl:ObjectProperty rdf:about="http://www.edmcouncil.org/spec/EDMC-SR/FND/Relative/ToolsAndInstruments/purposiveAmountIsApplicationOf">
      <skos:definition>The amount of something which is identified for the purpose, and which takes the form of some quantified resource. Scope Note: This may be an amount of capital, and amount of raw material etc. However, note that "Raw Material" may be regarded in one of two ways: as a possible resource to purchase, sell or store, or as a resource required specifically for some activity. The former is an Economic Resource, the latter a Purposive Amount.</skos:definition>
      <rdfs:subPropertyOf rdf:resource="http://www.edmcouncil.org/spec/EDMC-SR/FND/Relative/ToolsAndInstruments/isApplicationOf"/>
      <rdfs:domain rdf:resource="http://www.edmcouncil.org/spec/EDMC-SR/FND/Relative/ToolsAndInstruments/PurposiveAmount"/>
      <rdfs:range rdf:resource="http://www.edmcouncil.org/spec/EDMC-SR/FND/Relative/QuantifiedResources/QuantifiedResource"/>
   </owl:ObjectProperty>

   <owl:ObjectProperty rdf:about="http://www.edmcouncil.org/spec/EDMC-SR/FND/Relative/ToolsAndInstruments/rawMaterialIsApplicationOf">
      <skos:definition>The amount of material which is identified for the purpose, identified as a kind of economic resource.</skos:definition>
      <rdfs:subPropertyOf rdf:resource="http://www.edmcouncil.org/spec/EDMC-SR/FND/Relative/ToolsAndInstruments/purposiveAmountIsApplicationOf"/>
      <rdfs:domain rdf:resource="http://www.edmcouncil.org/spec/EDMC-SR/FND/Relative/ToolsAndInstruments/RawMaterial"/>
      <rdfs:range rdf:resource="http://www.edmcouncil.org/spec/EDMC-SR/FND/Relative/QuantifiedResources/QuantifiedRawMaterial"/>
   </owl:ObjectProperty>

   <owl:ObjectProperty rdf:about="http://www.edmcouncil.org/spec/EDMC-SR/FND/Relative/ToolsAndInstruments/toolIsApplicationOf">
      <skos:definition>The physical thing which is used as this tool.</skos:definition>
      <rdfs:subPropertyOf rdf:resource="http://www.edmcouncil.org/spec/EDMC-SR/FND/Relative/ToolsAndInstruments/isApplicationOf"/>
      <rdfs:domain rdf:resource="http://www.edmcouncil.org/spec/EDMC-SR/FND/Relative/ToolsAndInstruments/Tool"/>
      <rdfs:range rdf:resource="http://www.edmcouncil.org/spec/EDMC-SR/UO/Lattice/Concrete"/>
   </owl:ObjectProperty>

   <owl:ObjectProperty rdf:about="http://www.edmcouncil.org/spec/EDMC-SR/FND/Relative/ToolsAndInstruments/hasPurpose">
      <skos:definition>The purpose for which the Purposive Thing is defined; the reason some thing, with some (usually independent) form, is defined as a Purposive Thing. The actual or intended usage to which the thing is put or may be put.</skos:definition>
      <rdfs:subPropertyOf rdf:resource="http://www.edmcouncil.org/spec/EDMC-SR/UO/OntologicalDegree/inContext"/>
      <rdfs:domain rdf:resource="http://www.edmcouncil.org/spec/EDMC-SR/FND/Relative/ToolsAndInstruments/PurposiveThing"/>
      <rdfs:range rdf:resource="http://www.edmcouncil.org/spec/EDMC-SR/FND/Relative/ToolsAndInstruments/Purpose"/>
   </owl:ObjectProperty>

   <owl:ObjectProperty rdf:about="http://www.edmcouncil.org/spec/EDMC-SR/FND/Relative/ToolsAndInstruments/isApplicationOf">
      <skos:definition>The actual form of the Purposive Thing; the thing which is defined according to its purpose and is employed for that purpose. Editorial Note: This would usually be some Independent Thing. However it is conceivable that the existence of some relative thing, For example an asset, may itself be put to a purpose over and above the role or context already defined for it, and wholly dependent on it being that relative thing and not simply a thing in itself. Therefore this identity relationship has a range of Thing, but is modeled as a sub property of "identity" to make this conclusion explicit. This relationship need not be used in operational application ontologies as it adds no new logical assertion.</skos:definition>
      <rdfs:subPropertyOf rdf:resource="http://www.edmcouncil.org/spec/EDMC-SR/UO/OntologicalDegree/identity"/>
      <rdfs:domain rdf:resource="http://www.edmcouncil.org/spec/EDMC-SR/FND/Relative/ToolsAndInstruments/PurposiveThing"/>
      <rdfs:range rdf:resource="http://www.w3.org/2002/07/owl#Thing"/>
   </owl:ObjectProperty>

   <owl:ObjectProperty rdf:about="http://www.edmcouncil.org/spec/EDMC-SR/FND/Relative/ToolsAndInstruments/purposiveAmountHasPurpose">
      <skos:definition>The purpose for which the amount of something is intended to be used. Explanatory Note: This may be manufacturing investment etc. Scope Note: This may be further specialized or restricted to describe various manufacturing purposes (via or as restrictions on Raw Material), or various investment purposes for Investment Capital.</skos:definition>
      <rdfs:subPropertyOf rdf:resource="http://www.edmcouncil.org/spec/EDMC-SR/FND/Relative/ToolsAndInstruments/hasPurpose"/>
      <rdfs:domain rdf:resource="http://www.edmcouncil.org/spec/EDMC-SR/FND/Relative/ToolsAndInstruments/PurposiveAmount"/>
      <rdfs:range rdf:resource="http://www.edmcouncil.org/spec/EDMC-SR/FND/Relative/ToolsAndInstruments/Purpose"/>
   </owl:ObjectProperty>

   <!--Data Properties-->

<!--Annotation Properties-->

<!--Classes-->

<owl:Class rdf:about="http://www.edmcouncil.org/spec/EDMC-SR/FND/Relative/ToolsAndInstruments/FinancialInstrument">
      <rdfs:label>Financial Instrument</rdfs:label>
      <skos:definition>Some financial contract or agreement, described in the context of its use in furthering some investment purpose. Explanatory Note: This is specific to its usage. The term "Financial Instrument" is frequently applied to the contract (as a thing), which might be put to such purpose, rather than to the instrument as it is used as an instrument, which is what is defined by this concept.</skos:definition>
      <rdfs:subClassOf rdf:resource="http://www.edmcouncil.org/spec/EDMC-SR/FND/Relative/ToolsAndInstruments/Instrument"/>
   </owl:Class>

   <owl:Class rdf:about="http://www.edmcouncil.org/spec/EDMC-SR/FND/Relative/ToolsAndInstruments/Instrument">
      <rdfs:label>Instrument</rdfs:label>
      <skos:definition>Something which is used to further some purpose or to measure some variable in furtherance of some purpose. Explanatory Note: This may include more abstract or even relative or mediating things such as contracts, put to some purpose. For example, financial instruments. It also include physical measurement instruments (flow meters etc.) in industrial plant.</skos:definition>
      <rdfs:subClassOf rdf:resource="http://www.edmcouncil.org/spec/EDMC-SR/FND/Relative/ToolsAndInstruments/PurposiveThing"/>
   </owl:Class>

   <owl:Class rdf:about="http://www.edmcouncil.org/spec/EDMC-SR/FND/Relative/ToolsAndInstruments/MeasurementInstrument">
      <rdfs:label>Measurement Instrument</rdfs:label>
      <skos:definition>An instrument whose purpose is to measure some variable, for example in some physical process.</skos:definition>
   </owl:Class>

   <owl:Class rdf:about="http://www.edmcouncil.org/spec/EDMC-SR/FND/Relative/ToolsAndInstruments/MeasurementPurpose">
      <rdfs:label>Measurement Purpose</rdfs:label>
      <skos:definition>The purpose of measuring things.</skos:definition>
      <rdfs:subClassOf rdf:resource="http://www.edmcouncil.org/spec/EDMC-SR/FND/Relative/ToolsAndInstruments/Purpose"/>
   </owl:Class>

   <owl:Class rdf:about="http://www.edmcouncil.org/spec/EDMC-SR/FND/Relative/ToolsAndInstruments/Purpose">
      <rdfs:label>Purpose</rdfs:label>
      <skos:definition>The context in which some thing is, may be or is planned to be put to some use by someone.</skos:definition>
      <rdfs:subClassOf rdf:resource="http://www.edmcouncil.org/spec/EDMC-SR/UO/OntologicalDegree/MediatingThing"/>
   </owl:Class>

   <owl:Class rdf:about="http://www.edmcouncil.org/spec/EDMC-SR/FND/Relative/ToolsAndInstruments/PurposiveAmount">
      <rdfs:label>Purposive Amount</rdfs:label>
      <skos:definition>An amount of something defined in terms of its usefulness for some purpose. Scope Note: Includes investment capital (an amount of capital intended or used for investment), and amounts of raw material used or to be used in e.g. manufacture of something.</skos:definition>
   </owl:Class>

   <owl:Class rdf:about="http://www.edmcouncil.org/spec/EDMC-SR/FND/Relative/ToolsAndInstruments/PurposiveThing">
      <rdfs:label>Purposive Thing</rdfs:label>
      <skos:definition>Something described in terms of its purpose or potential purpose. Editorial Note: That which fulfils this role is generally taken to be some kind of Independent Thing However it is conceivable that the existence of some relative thing, for example an asset, may itself be put to a purpose over and above the role or context already defined for it, and wholly dependent on it being that relative thing and not siply a thing in itself. therefore the identity relationship is modeled with a range of Thing, but is modeled as a separate relationship to that of Relative Thing in order to make this conclusion explicit. This relationship need not be used in operational application ontologies as it adds no new logical assertion.</skos:definition>
      <rdfs:subClassOf rdf:resource="http://www.edmcouncil.org/spec/EDMC-SR/UO/OntologicalDegree/RelativeThing"/>
   </owl:Class>

   <owl:Class rdf:about="http://www.edmcouncil.org/spec/EDMC-SR/FND/Relative/ToolsAndInstruments/RawMaterial">
      <rdfs:label>Raw Material</rdfs:label>
      <skos:definition>An amount of some material intended to be used for some purpose e.g. in manufacture, refinery. Scope Note: This is out of scope for financial services applications (unless it is needed for various loan purposes). This may be implemented in manufacturing models to define various manufacturing and refinement purposes, but at this level it is more general than any one of those.</skos:definition>
      <rdfs:subClassOf rdf:resource="http://www.edmcouncil.org/spec/EDMC-SR/FND/Relative/ToolsAndInstruments/PurposiveAmount"/>
   </owl:Class>

   <owl:Class rdf:about="http://www.edmcouncil.org/spec/EDMC-SR/FND/Relative/ToolsAndInstruments/Tool">
      <rdfs:label>Tool</rdfs:label>
      <skos:definition>Some physical object which is put to some purpose.</skos:definition>
   </owl:Class>

   <!--Individuals-->

</rdf:RDF>