<?xml version="1.0" encoding="UTF-8"?>
  
<!DOCTYPE rdf:RDF [
    <!ENTITY fibo-ind-ind-ind "http://spec.edmcouncil.org/fibo/red/ind/indicators/indicators/">
    <!ENTITY fibo-fnd-pub-pub "http://spec.edmcouncil.org/fibo/red/fnd/publications/publications/">
    <!ENTITY fibo-fnd-math-math "http://spec.edmcouncil.org/fibo/red/fnd/math/math/">
    <!ENTITY fibo-fnd-rel-rel "http://spec.edmcouncil.org/fibo/red/fnd/relations/relations/">
    <!ENTITY fibo-be-le-fbo "http://spec.edmcouncil.org/fibo/red/be/legal-entities/formal-business-organizations/">
    <!ENTITY  "http://spec.edmcouncil.org/fibo/red/fnd/utilities/">
    <!ENTITY fibo-md-tmp-ins "http://spec.edmcouncil.org/fibo/red/md/temporal-core/instrument-temporal-terms/">
]>

<rdf:RDF xmlns:xsd="http://www.w3.org/2001/XMLSchema#"
         xmlns:sm="http://www.omg.org/techprocess/ab/SpecificationMetadata/"
         xmlns:xs="http://www.w3.org/2001/XMLSchema"
         xmlns:fibo-fnd-utl-av="http://www.omg.org/spec/EDMC-FIBO/FND/Utilities/AnnotationVocabulary/"
         xmlns:rdf="http://www.w3.org/1999/02/22-rdf-syntax-ns#"
         xmlns:rdfs="http://www.w3.org/2000/01/rdf-schema#"
         xmlns:owl="http://www.w3.org/2002/07/owl#"
         xmlns:skos="http://www.w3.org/2004/02/skos/core#"
         xmlns:dc="http://purl.org/dc/terms/"
         xml:base="http://spec.edmcouncil.org/fibo/red/ind/indicators/indicators/">

   <owl:Ontology rdf:about="http://spec.edmcouncil.org/fibo/red/ind/indicators/indicators/">
      <owl:imports rdf:resource="http://spec.edmcouncil.org/fibo/red/fnd/publications/publications/"/>
      <owl:imports rdf:resource="http://spec.edmcouncil.org/fibo/red/fnd/math/math/"/>
      <owl:imports rdf:resource="http://spec.edmcouncil.org/fibo/red/fnd/relations/relations/"/>
      <owl:imports rdf:resource="http://spec.edmcouncil.org/fibo/red/be/legal-entities/formal-business-organizations/"/>
      <owl:imports rdf:resource="http://spec.edmcouncil.org/fibo/red/fnd/utilities/analytics"/>
      <owl:imports rdf:resource="http://spec.edmcouncil.org/fibo/red/md/temporal-core/instrument-temporal-terms/"/>
   </owl:Ontology>


  <!--
    ///////////////////////////////////////////////////////////////////////////////////////
    //
    // Datatypes
    //
    ///////////////////////////////////////////////////////////////////////////////////////
    -->



  <!--
    ///////////////////////////////////////////////////////////////////////////////////////
    //
    // Object Properties
    //
    ///////////////////////////////////////////////////////////////////////////////////////
    -->


<owl:ObjectProperty rdf:about="&fibo-ind-ind-ind;financialInformationPublisherHasIdentity">
      <rdfs:label>financial information publisher has identity</rdfs:label>
      <rdfs:subPropertyOf rdf:resource="&fibo-fnd-pub-pub;publisherIdentity"/>
      <rdfs:domain rdf:resource="&fibo-ind-ind-ind;FinancialInformationPublisher"/>
      <rdfs:range rdf:resource="&fibo-be-le-fbo;FormallyConstitutedOrganization"/>
   </owl:ObjectProperty>

   <owl:ObjectProperty rdf:about="&fibo-ind-ind-ind;marketSpreadIsBetween">
      <rdfs:label>market spread is between</rdfs:label>
      <rdfs:subPropertyOf rdf:resource="http://spec.edmcouncil.org/fibo/red/fnd/utilities/analytics/"/>
      <rdfs:subPropertyOf rdf:resource="&fibo-md-tmp-ins;spreadIsBetween"/>
      <rdfs:domain rdf:resource="&fibo-ind-ind-ind;MarketSpread"/>
      <rdfs:range rdf:resource="&fibo-ind-ind-ind;MarketReferentialParameter"/>
   </owl:ObjectProperty>

   <owl:ObjectProperty rdf:about="&fibo-ind-ind-ind;isVolatilityOf">
      <rdfs:label>is volatility of</rdfs:label>
      <skos:definition>The market rate to which the volatility measure applies and of which it is a measure.</skos:definition>
      <rdfs:subPropertyOf rdf:resource="&fibo-fnd-math-math;parameterAppliesTo"/>
      <rdfs:subPropertyOf rdf:resource="&fibo-fnd-rel-rel;appliesTo"/>
      <rdfs:domain rdf:resource="&fibo-ind-ind-ind;Volatility"/>
      <rdfs:range rdf:resource="&fibo-ind-ind-ind;MarketBaseRate"/>
   </owl:ObjectProperty>

   <owl:ObjectProperty rdf:about="&fibo-ind-ind-ind;isPublishedBy">
      <rdfs:label>is published by</rdfs:label>
      <rdfs:subPropertyOf rdf:resource="&fibo-fnd-rel-rel;isProvidedBy"/>
      <rdfs:subPropertyOf rdf:resource="&fibo-fnd-pub-pub;publishedBy"/>
      <rdfs:domain rdf:resource="&fibo-ind-ind-ind;MarketReferentialParameter"/>
      <rdfs:range rdf:resource="&fibo-ind-ind-ind;FinancialInformationPublisher"/>
      <owl:inverseOf rdf:resource="&fibo-ind-ind-ind;publishes"/>
   </owl:ObjectProperty>

   <owl:ObjectProperty rdf:about="&fibo-ind-ind-ind;publishes">
      <rdfs:label>publishes</rdfs:label>
      <skos:definition>Information published by the publisher, in the form of some market referential parameter such as an economic index or indicator.</skos:definition>
      <rdfs:subPropertyOf rdf:resource="&fibo-fnd-rel-rel;provides"/>
      <rdfs:domain rdf:resource="&fibo-ind-ind-ind;FinancialInformationPublisher"/>
      <rdfs:range rdf:resource="&fibo-ind-ind-ind;MarketReferentialParameter"/>
   </owl:ObjectProperty>


  <!--
    ///////////////////////////////////////////////////////////////////////////////////////
    //
    // Data Properties
    //
    ///////////////////////////////////////////////////////////////////////////////////////
    -->



  <!--
    ///////////////////////////////////////////////////////////////////////////////////////
    //
    // Annotation Properties
    //
    ///////////////////////////////////////////////////////////////////////////////////////
    -->



  <!--
    ///////////////////////////////////////////////////////////////////////////////////////
    //
    // Classes
    //
    ///////////////////////////////////////////////////////////////////////////////////////
    -->


<owl:Class rdf:about="&fibo-ind-ind-ind;FinancialInformationPublisher">
      <rdfs:label>financial information publisher</rdfs:label>
      <skos:definition>Some entity which is acting in the capacity of a publisher or provider of information relating to the financial markets, or information which is of interest to those markets including information on economies, governments etc.</skos:definition>
      <rdfs:subClassOf rdf:resource="&fibo-fnd-pub-pub;Publisher"/>
   </owl:Class>

   <owl:Class rdf:about="&fibo-ind-ind-ind;MarketBaseRate">
      <rdfs:label>market base rate</rdfs:label>
      <skos:definition>Calculated notional value used to measure market trends for a set of instruments (S&amp;P500, NASDAQ composite, 30day CD) or express economical climate for an industry (DowJones Industrial, H&amp;Q Growth Technologies) and/or political region (Libor, Prime)</skos:definition>
      <rdfs:subClassOf rdf:resource="&fibo-ind-ind-ind;MarketReferentialParameter"/>
   </owl:Class>

   <owl:Class rdf:about="&fibo-ind-ind-ind;MarketReferentialParameter">
      <rdfs:label>market referential parameter</rdfs:label>
      <skos:definition>A published parameter about financial or other markets, such as an index, an indicator or an interest rate.</skos:definition>
      <rdfs:subClassOf rdf:resource="&fibo-md-tmp-ins;FinancialMarketInformation"/>
      <rdfs:subClassOf rdf:resource="&fibo-fnd-math-math;TimedParameter"/>
   </owl:Class>

   <owl:Class rdf:about="&fibo-ind-ind-ind;MarketSpread">
      <rdfs:label>market spread</rdfs:label>
      <skos:definition>A published spread between some two market rates.</skos:definition>
      <rdfs:subClassOf rdf:resource="&fibo-md-tmp-ins;Spread"/>
   </owl:Class>

   <owl:Class rdf:about="&fibo-ind-ind-ind;Volatility">
      <rdfs:label>volatility</rdfs:label>
      <skos:definition>A measure of security price fluctuation. Mathematically the volatility is the annualized standard deviation of a security's daily price changes</skos:definition>
   </owl:Class>


  <!--
    ///////////////////////////////////////////////////////////////////////////////////////
    //
    // Individuals
    //
    ///////////////////////////////////////////////////////////////////////////////////////
    -->


</rdf:RDF>