<?xml version="1.0" encoding="UTF-8"?>
<rdf:RDF xmlns:xsd="http://www.w3.org/2001/XMLSchema#"
         xmlns:sm="http://www.omg.org/techprocess/ab/SpecificationMetadata/"
         xmlns:fibo-fnd-utl-av="http://www.omg.org/spec/EDMC-FIBO/FND/Utilities/AnnotationVocabulary/"
         xmlns:rdf="http://www.w3.org/1999/02/22-rdf-syntax-ns#"
         xmlns:rdfs="http://www.w3.org/2000/01/rdf-schema#"
         xmlns:owl="http://www.w3.org/2002/07/owl#"
         xmlns:skos="http://www.w3.org/2004/02/skos/core#"
         xmlns:dc="http://purl.org/dc/terms/"
         xml:base="http://www.omg.org/spec/EDMC-SR/BE/Corporations/Corporations/">

   <owl:Ontology rdf:about="http://www.omg.org/spec/EDMC-SR/BE/Corporations/Corporations/">
      <owl:imports rdf:resource="http://www.omg.org/spec/EDMC-SR/BE/LegalEntities/CorporateBodies/"/>
      <owl:imports rdf:resource="http://www.omg.org/spec/EDMC-SR/BE/LegalEntities/FormalBusinessOrganizations/"/>
      <owl:imports rdf:resource="http://www.omg.org/spec/EDMC-SR/BE/LegalEntities/LegalPersons/"/>
   </owl:Ontology>

   <!--Datatypes-->

<!--Object Properties-->

<owl:ObjectProperty rdf:about="http://www.omg.org/spec/EDMC-SR/BE/Corporations/Corporations/incorporatedCompanyHasIssuedCapital">
      <skos:definition>The amount of equity in the company, which has been issued in the form of shares (either publicly traded or privately held).</skos:definition>
      <rdfs:subPropertyOf rdf:resource="http://www.omg.org/spec/EDMC-SR/BE/Corporations/Corporations/hasIssuedCapital"/>
      <rdfs:domain rdf:resource="http://www.omg.org/spec/EDMC-SR/BE/Corporations/Corporations/IncorporatedCompany"/>
      <rdfs:range rdf:resource="http://www.omg.org/spec/FIBO/Foundation/Accounting/CurrencyAmount/MonetaryAmount"/>
   </owl:ObjectProperty>

   <owl:ObjectProperty rdf:about="http://www.omg.org/spec/EDMC-SR/BE/Corporations/Corporations/incorporatedCompanyHasNominalCapital">
      <skos:definition>The total amount of capital which the company is authorized to issue as equity in the form of shares, according to the company's legal documentation (Memorandum and Articles, or equivalent).</skos:definition>
      <rdfs:subPropertyOf rdf:resource="http://www.omg.org/spec/EDMC-SR/BE/Corporations/Corporations/hasNominalCapital"/>
      <rdfs:domain rdf:resource="http://www.omg.org/spec/EDMC-SR/BE/Corporations/Corporations/IncorporatedCompany"/>
      <rdfs:range rdf:resource="http://www.omg.org/spec/FIBO/Foundation/Accounting/CurrencyAmount/MonetaryAmount"/>
   </owl:ObjectProperty>

   <owl:ObjectProperty rdf:about="http://www.omg.org/spec/EDMC-SR/BE/Corporations/Corporations/governedByBoardAgreement">
      <skos:definition>The agreement which covers the relationships among the Board Members and between them and the Corporation as a legal entity.</skos:definition>
      <rdfs:subPropertyOf rdf:resource="http://www.omg.org/spec/EDMC-SR/BE/LegalEntities/FormalBusinessOrganizations/formallyConstitutedOrganizationIsGovernedBy"/>
      <rdfs:domain rdf:resource="http://www.omg.org/spec/EDMC-SR/BE/Corporations/Corporations/IncorporatedCompany"/>
      <rdfs:range rdf:resource="http://www.omg.org/spec/EDMC-SR/BE/Corporations/Corporations/BoardAgreement"/>
   </owl:ObjectProperty>

   <owl:ObjectProperty rdf:about="http://www.omg.org/spec/EDMC-SR/BE/Corporations/Corporations/hasIssuedCapital">
      <skos:definition>The total of a companys shares that are held by shareholders. A company can, at any time, issue new shares up to the full amount of authorized share capital.</skos:definition>
      <rdfs:subPropertyOf rdf:resource="http://www.omg.org/spec/EDMC-SR/BE/Corporations/Corporations/hasNominalCapital"/>
      <rdfs:domain rdf:resource="http://www.omg.org/spec/EDMC-SR/FND/Relations/Relations/Thing"/>
      <rdfs:range rdf:resource="http://www.omg.org/spec/FIBO/Foundation/Accounting/CurrencyAmount/MonetaryAmount"/>
   </owl:ObjectProperty>

   <owl:ObjectProperty rdf:about="http://www.omg.org/spec/EDMC-SR/BE/Corporations/Corporations/hasNominalCapital">
      <skos:definition>Nominal capital is an alternate term for authorized share capital. The maximum value of securities that a company can legally issue. This number is specified in the memorandum of association (or articles of incorporation in the US) when a company is incorporated, but can be changed later with shareholders approval. Authorized share capital may be divided into (1) Issued capital - par value of the shares actually issued, (2) Paid up capital - money received from the shareholders in exchange for shares, and (3) Uncalled capital - money remaining unpaid by the shareholders for the shares they have bought.</skos:definition>
      <rdfs:domain rdf:resource="http://www.omg.org/spec/EDMC-SR/FND/Relations/Relations/Thing"/>
      <rdfs:range rdf:resource="http://www.omg.org/spec/FIBO/Foundation/Accounting/CurrencyAmount/MonetaryAmount"/>
   </owl:ObjectProperty>

   <owl:ObjectProperty rdf:about="http://www.omg.org/spec/EDMC-SR/BE/Corporations/Corporations/allocatedUnder">
      <skos:definition>The jurisdiction under which the registration code is allocated.</skos:definition>
      <rdfs:subPropertyOf rdf:resource="http://www.omg.org/spec/EDMC-SR/FND/Relations/Relations/isGoverneBy"/>
      <rdfs:domain rdf:resource="http://www.omg.org/spec/EDMC-SR/BE/Corporations/Corporations/CompanyRegistrationCode"/>
      <rdfs:range rdf:resource="http://www.omg.org/spec/EDMC-SR/FND/Law/Jurisdictions/Jurisdiction"/>
   </owl:ObjectProperty>

   <owl:ObjectProperty rdf:about="http://www.omg.org/spec/EDMC-SR/BE/Corporations/Corporations/hasRegistrationCode">
      <skos:definition>The official registration number of the incorporated company in the Jurisdiction in which it is registered.</skos:definition>
      <skos:editorialNote>Editorial Note: It was suggested that some jurisdictions do not insist on the existence of such a number, so this was given as optional. It is now tightened to mandatory (cardinality = 1)</skos:editorialNote>
      <rdfs:subPropertyOf rdf:resource="http://www.omg.org/spec/EDMC-SR/FND/Relations/Relations/isIdentifiedBy"/>
      <rdfs:domain rdf:resource="http://www.omg.org/spec/EDMC-SR/BE/Corporations/Corporations/IncorporatedCompany"/>
      <rdfs:range rdf:resource="http://www.omg.org/spec/EDMC-SR/BE/Corporations/Corporations/CompanyRegistrationCode"/>
   </owl:ObjectProperty>

   <!--Data Properties-->

<owl:DatatypeProperty rdf:about="http://www.omg.org/spec/EDMC-SR/BE/Corporations/Corporations/hasDateOfIncorporation">
      <rdfs:range rdf:resource="http://www.w3.org/2001/XMLSchema#date"/>
   </owl:DatatypeProperty>

   <owl:DatatypeProperty rdf:about="http://www.omg.org/spec/EDMC-SR/BE/Corporations/Corporations/hasDateOfRegistration">
      <rdfs:range rdf:resource="http://www.w3.org/2001/XMLSchema#date"/>
   </owl:DatatypeProperty>

   <owl:DatatypeProperty rdf:about="http://www.omg.org/spec/EDMC-SR/BE/Corporations/Corporations/hasLegalFormAbbreviation">
      <rdfs:range rdf:resource="http://www.omg.org/spec/EDMC-SR/FND/Utilities/BusinessFacingTypes/text"/>
   </owl:DatatypeProperty>

   <!--Annotation Properties-->

<!--Classes-->

<owl:Class rdf:about="http://www.omg.org/spec/EDMC-SR/BE/Corporations/Corporations/BoardAgreement">
      <rdfs:label>Board Agreement</rdfs:label>
      <skos:definition>The agreement between members of the Board of the Company.</skos:definition>
      <rdfs:subClassOf rdf:resource="http://www.omg.org/spec/EDMC-SR/BE/LegalEntities/FormalBusinessOrganizations/OrganizationCoveringAgreement"/>
   </owl:Class>

   <owl:Class rdf:about="http://www.omg.org/spec/EDMC-SR/BE/Corporations/Corporations/JointStockCompany">
      <rdfs:label>Joint Stock Company</rdfs:label>
      <skos:definition>A joint stock company (JSC) is a type of business entity: it is a type of corporation or partnership between two companies. Certificates of ownership (or stocks) are issued by the company in return for each contribution, and the shareholders are free to transfer their ownership interest at any time by selling their stockholding to others.</skos:definition>
      <skos:editorialNote>There are two kinds of joint stock company. The private company kind and the open market. The shares are usually only held by the directors and Company Secretary.</skos:editorialNote>
      <rdfs:subClassOf rdf:resource="http://www.omg.org/spec/EDMC-SR/BE/Corporations/Corporations/IncorporatedCompany"/>
   </owl:Class>

   <owl:Class rdf:about="http://www.omg.org/spec/EDMC-SR/BE/Corporations/Corporations/PrivatelyHeldCompany">
      <rdfs:label>Privately Held Company</rdfs:label>
      <skos:definition>A company whose shares are held privately, usually by the directors or their relatives and associates.</skos:definition>
      <skos:editorialNote>Wikipedia: definition for British / Commonwealth version: A private company limited by shares is a type of company incorporated under the laws of England and Wales, Scotland, that of certain Commonwealth countries and the Republic of Ireland. It has shareholders with limited liability and its shares may not be offered to the general public, unlike those of public limited companies. Additional notes from Wikipedia "Limited by shares" means that the company has shareholders, and that the liability of the shareholders to creditors of the company is limited to the capital originally invested, i.e. the nominal value of the shares and any premium paid in return for the issue of the shares by the company. A shareholder's personal assets are thereby protected in the event of the company's insolvency, but money invested in the company will be lost. A limited company may be "private" or "public". A private limited company's disclosure requirements are lighter, but for this reason its shares may not be offered to the general public (and therefore cannot be traded on a public stock exchange). This is the major distinguishing feature between a private limited company and a public limited company. Most companies, particularly small companies, are private. Private companies limited by shares are required to have the suffix "Limited" (often written "Ltd" or "Ltd.") or "Incorporated" ("Inc.") as part of their name, though the latter cannot be used in the UK or the Republic of Ireland. In the Republic of Ireland "Teoranta" ("Teo.") may be used instead, largely by Gaeltacht companies. "Cyfyngedig" ("Cyf.") may be used by Welsh companies in a similar fashion. term Origin:EDMC Reviews</skos:editorialNote>
   </owl:Class>

   <owl:Class rdf:about="http://www.omg.org/spec/EDMC-SR/BE/Corporations/Corporations/PubliclyHeldCompany">
      <rdfs:label>Publicly Held Company</rdfs:label>
      <skos:definition>A company whose shares are traded and held publicly.</skos:definition>
      <skos:editorialNote>SME Review 16 Feb 2011. Separate "Public" in definition of company, from publicly traded shares - not related.</skos:editorialNote>
   </owl:Class>

   <owl:Class rdf:about="http://www.omg.org/spec/EDMC-SR/BE/Corporations/Corporations/CompanyRegistrationCode">
      <rdfs:label>Company Registration Code</rdfs:label>
      <skos:definition>A code which is officially allocated under a jurisdiction in which a company is incorporated, and which is used within that jurisdiction to identify the company. This usually has to be included in official stationery and must always be publicly available.</skos:definition>
      <rdfs:subClassOf rdf:resource="http://www.omg.org/spec/EDMC-SR/BE/LegalEntities/FormalBusinessOrganizations/OrganizationIdentificationCode"/>
      <rdfs:subClassOf rdf:resource="http://www.edmcouncil.org/spec/EDMC-SR/FND/Information/Schemes/RegistrationCode"/>
   </owl:Class>

   <owl:Class rdf:about="http://www.omg.org/spec/EDMC-SR/BE/Corporations/Corporations/IncorporatedCompany">
      <rdfs:label>Incorporated Company</rdfs:label>
      <skos:definition>A company incorporated by the issue of shares.</skos:definition>
      <rdfs:subClassOf rdf:resource="http://www.omg.org/spec/EDMC-SR/BE/LegalEntities/CorporateBodies/BodyIncorporatedWithEquity"/>
   </owl:Class>

   <!--Individuals-->

</rdf:RDF>