<?xml version="1.0" encoding="UTF-8"?>
  
<!DOCTYPE rdf:RDF [
    <!ENTITY fibo-fnd-lawx-jur "http://spec.edmcouncil.org/fibo/red/fnd/law-ext/jurisdiction-extended/">
    <!ENTITY fibo-uo-rl "http://spec.edmcouncil.org/fibo/red/uo/relatives/">
    <!ENTITY fibo-fnd-law-cor "http://spec.edmcouncil.org/fibo/red/fnd/law/legal-core/">
    <!ENTITY fibo-fnd-law-jur "http://spec.edmcouncil.org/fibo/red/fnd/law/jurisdictions/">
]>

<rdf:RDF xmlns:xsd="http://www.w3.org/2001/XMLSchema#"
         xmlns:sm="http://www.omg.org/techprocess/ab/SpecificationMetadata/"
         xmlns:xs="http://www.w3.org/2001/XMLSchema"
         xmlns:fibo-fnd-utl-av="http://www.omg.org/spec/EDMC-FIBO/FND/Utilities/AnnotationVocabulary/"
         xmlns:rdf="http://www.w3.org/1999/02/22-rdf-syntax-ns#"
         xmlns:rdfs="http://www.w3.org/2000/01/rdf-schema#"
         xmlns:owl="http://www.w3.org/2002/07/owl#"
         xmlns:skos="http://www.w3.org/2004/02/skos/core#"
         xmlns:dc="http://purl.org/dc/terms/"
         xml:base="http://spec.edmcouncil.org/fibo/red/fnd/law-ext/jurisdiction-extended/">

   <owl:Ontology rdf:about="http://spec.edmcouncil.org/fibo/red/fnd/law-ext/jurisdiction-extended/">
      <owl:imports rdf:resource="http://spec.edmcouncil.org/fibo/red/uo/relatives/"/>
      <owl:imports rdf:resource="http://spec.edmcouncil.org/fibo/red/fnd/law/legal-core/"/>
      <owl:imports rdf:resource="http://spec.edmcouncil.org/fibo/red/fnd/law/jurisdictions/"/>
   </owl:Ontology>


  <!--
    ///////////////////////////////////////////////////////////////////////////////////////
    //
    // Datatypes
    //
    ///////////////////////////////////////////////////////////////////////////////////////
    -->



  <!--
    ///////////////////////////////////////////////////////////////////////////////////////
    //
    // Object Properties
    //
    ///////////////////////////////////////////////////////////////////////////////////////
    -->


<owl:ObjectProperty rdf:about="&fibo-fnd-lawx-jur;bijuridicialJurisdictionPartiallyGovernedUnderCivilLawSystem">
      <rdfs:label>bijuridicial jurisdiction partially governed under civil law system</rdfs:label>
      <skos:definition>One system of law under which a Bijuridicial Jurisdiction is governed is the system of Civil Law.</skos:definition>
      <rdfs:subPropertyOf rdf:resource="&fibo-fnd-law-jur;jurisdictionGovernedBy"/>
      <rdfs:domain rdf:resource="&fibo-fnd-lawx-jur;BijuridicialJurisdiction"/>
      <rdfs:range rdf:resource="&fibo-fnd-law-jur;CivilLawSystem"/>
   </owl:ObjectProperty>

   <owl:ObjectProperty rdf:about="&fibo-fnd-lawx-jur;bijuridicialJurisdictionPartiallyGovernedUnderCommonLawSystem">
      <rdfs:label>bijuridicial jurisdiction partially governed under common law system</rdfs:label>
      <skos:definition>One system of law under which a Bijuridicial Jurisdiction is governed is the system of Common Law.</skos:definition>
      <rdfs:subPropertyOf rdf:resource="&fibo-fnd-law-jur;jurisdictionGovernedBy"/>
      <rdfs:domain rdf:resource="&fibo-fnd-lawx-jur;BijuridicialJurisdiction"/>
      <rdfs:range rdf:resource="&fibo-fnd-law-jur;CommonLawSystem"/>
   </owl:ObjectProperty>

   <owl:ObjectProperty rdf:about="&fibo-fnd-lawx-jur;incorporatesSome">
      <rdfs:label>incorporates some</rdfs:label>
      <skos:definition>The laws included in this Body of Law.</skos:definition>
      <rdfs:domain rdf:resource="&fibo-fnd-lawx-jur;BodyOfLaw"/>
      <rdfs:range rdf:resource="&fibo-fnd-law-cor;Law"/>
   </owl:ObjectProperty>

   <owl:ObjectProperty rdf:about="&fibo-fnd-lawx-jur;hasInForce">
      <rdfs:label>has in force</rdfs:label>
      <rdfs:domain rdf:resource="&fibo-fnd-law-jur;Jurisdiction"/>
      <rdfs:range rdf:resource="&fibo-fnd-law-jur;StatuteLaw"/>
      <owl:inverseOf rdf:resource="&fibo-fnd-law-jur;isInForceIn"/>
   </owl:ObjectProperty>

   <owl:ObjectProperty rdf:about="&fibo-fnd-lawx-jur;definesTheApplicationOf">
      <rdfs:label>defines the application of</rdfs:label>
      <skos:definition>The Body of Law, the application of which is defined in the Legal System.</skos:definition>
      <rdfs:domain rdf:resource="&fibo-fnd-law-jur;LegalSystem"/>
      <rdfs:range rdf:resource="&fibo-fnd-lawx-jur;BodyOfLaw"/>
   </owl:ObjectProperty>

   <owl:ObjectProperty rdf:about="&fibo-fnd-lawx-jur;religiousLawJurisdictionGovernedUnder">
      <rdfs:label>religious law jurisdiction governed under</rdfs:label>
      <skos:definition>The system of law under which a Religious Law Jurisdiction is governed. This is some system of Religious Law.</skos:definition>
      <rdfs:subPropertyOf rdf:resource="&fibo-fnd-law-jur;jurisdictionGovernedBy"/>
      <rdfs:domain rdf:resource="&fibo-fnd-lawx-jur;ReligiousLawJurisdiction"/>
      <rdfs:range rdf:resource="&fibo-fnd-lawx-jur;ReligiousLawSystem"/>
   </owl:ObjectProperty>

   <owl:ObjectProperty rdf:about="&fibo-fnd-lawx-jur;shariaLawJurisdictionGovernedUnder">
      <rdfs:label>sharia law jurisdiction governed under</rdfs:label>
      <skos:definition>The system of law under which a Shari'a Law Jurisdiction is governed. This is the system of Shari'a Law.</skos:definition>
      <rdfs:subPropertyOf rdf:resource="&fibo-fnd-lawx-jur;religiousLawJurisdictionGovernedUnder"/>
      <rdfs:domain rdf:resource="&fibo-fnd-lawx-jur;ShariaLawJurisdiction"/>
      <rdfs:range rdf:resource="&fibo-fnd-lawx-jur;ShariaLawSystem"/>
   </owl:ObjectProperty>

   <owl:ObjectProperty rdf:about="&fibo-fnd-lawx-jur;constrainsStatuteLaw">
      <rdfs:label>constrains statute law</rdfs:label>
      <skos:definition>The Constitution constrains what can or cannot be legislated as Law for the Jurisdiction in which that Constitution applies.</skos:definition>
      <rdfs:subPropertyOf rdf:resource="&fibo-fnd-law-cor;governs"/>
      <rdfs:domain rdf:resource="&fibo-fnd-law-cor;GovernmentalConstitution"/>
      <rdfs:range rdf:resource="&fibo-fnd-law-jur;StatuteLaw"/>
   </owl:ObjectProperty>

   <owl:ObjectProperty rdf:about="&fibo-fnd-lawx-jur;governsLegalSystem">
      <rdfs:label>governs legal system</rdfs:label>
      <rdfs:domain rdf:resource="&fibo-fnd-law-cor;GovernmentalConstitution"/>
      <rdfs:range rdf:resource="&fibo-fnd-law-jur;LegalSystem"/>
      <owl:inverseOf rdf:resource="&fibo-fnd-law-jur;legalSystemIsGovernedBy"/>
   </owl:ObjectProperty>


  <!--
    ///////////////////////////////////////////////////////////////////////////////////////
    //
    // Data Properties
    //
    ///////////////////////////////////////////////////////////////////////////////////////
    -->



  <!--
    ///////////////////////////////////////////////////////////////////////////////////////
    //
    // Annotation Properties
    //
    ///////////////////////////////////////////////////////////////////////////////////////
    -->



  <!--
    ///////////////////////////////////////////////////////////////////////////////////////
    //
    // Classes
    //
    ///////////////////////////////////////////////////////////////////////////////////////
    -->


<owl:Class rdf:about="&fibo-fnd-lawx-jur;BijuridicialJurisdiction">
      <rdfs:label>bijuridicial jurisdiction</rdfs:label>
      <skos:definition>A Jurisdiction in which two or more systems of law are in force.</skos:definition>
      <rdfs:subClassOf rdf:resource="&fibo-fnd-law-jur;Jurisdiction"/>
   </owl:Class>

   <owl:Class rdf:about="&fibo-fnd-lawx-jur;BodyOfLaw">
      <rdfs:label>body of law</rdfs:label>
      <skos:definition>Some body of law, that is some set of laws, statutes, ordinances and the like.</skos:definition>
      <rdfs:subClassOf rdf:resource="&fibo-uo-rl;IndependentThing"/>
   </owl:Class>

   <owl:Class rdf:about="&fibo-fnd-lawx-jur;CanonLawSystem">
      <rdfs:label>canon law system</rdfs:label>
      <skos:definition>The body of laws & regulations made or adopted by ecclesiastical authority, for the government of the Christian organization and its members.</skos:definition>
      <rdfs:subClassOf rdf:resource="&fibo-fnd-lawx-jur;ReligiousLawSystem"/>
   </owl:Class>

   <owl:Class rdf:about="&fibo-fnd-lawx-jur;CivilLaw">
      <rdfs:label>civil law</rdfs:label>
      <skos:definition>The branch of the law dealing with disputes between individuals or organizations, in which compensation may be awarded to the victim.</skos:definition>
      <rdfs:subClassOf rdf:resource="&fibo-fnd-lawx-jur;CommonLaw"/>
   </owl:Class>

   <owl:Class rdf:about="&fibo-fnd-lawx-jur;CommonLaw">
      <rdfs:label>common law</rdfs:label>
      <skos:definition>Law developed by judges through decisions of courts and similar tribunals rather than through legislative statutes or executive branch action.</skos:definition>
      <rdfs:subClassOf rdf:resource="&fibo-fnd-lawx-jur;BodyOfLaw"/>
   </owl:Class>

   <owl:Class rdf:about="&fibo-fnd-lawx-jur;ConstitutionalLaw">
      <rdfs:label>constitutional law</rdfs:label>
      <skos:definition>The body of law which defines the relationship of different entities within a state, namely the executive, legislature and the judiciary. Further notes: (from Wikipedia): Constitutional laws may be considered second order rulemaking or rules about making rules to exercise power.</skos:definition>
   </owl:Class>

   <owl:Class rdf:about="&fibo-fnd-lawx-jur;CriminalLaw">
      <rdfs:label>criminal law</rdfs:label>
      <skos:definition>The body of law that defines conduct that is not allowed because it is held to threaten, harm or endanger the safety and welfare of people, and that sets out the punishments to be imposed on people who do not obey these laws.</skos:definition>
   </owl:Class>

   <owl:Class rdf:about="&fibo-fnd-lawx-jur;InternationalLaw">
      <rdfs:label>international law</rdfs:label>
      <skos:definition>The set of rules generally regarded and accepted as binding in relations between states and nations.</skos:definition>
   </owl:Class>

   <owl:Class rdf:about="&fibo-fnd-lawx-jur;ReligiousLaw">
      <rdfs:label>religious law</rdfs:label>
      <skos:definition>Some set of laws derived from and practised in the name of some religion.</skos:definition>
   </owl:Class>

   <owl:Class rdf:about="&fibo-fnd-lawx-jur;ReligiousLawJurisdiction">
      <rdfs:label>religious law jurisdiction</rdfs:label>
      <skos:definition>A Jurisdiction in which some system of religious law is in force.</skos:definition>
   </owl:Class>

   <owl:Class rdf:about="&fibo-fnd-lawx-jur;ReligiousLawSystem">
      <rdfs:label>religious law system</rdfs:label>
      <skos:definition>Some system of law based on the ordering principle of reality as being knowledge as revealed by God and governing all human affairs.</skos:definition>
      <rdfs:subClassOf rdf:resource="&fibo-fnd-law-jur;LegalSystem"/>
   </owl:Class>

   <owl:Class rdf:about="&fibo-fnd-lawx-jur;ShariaLawJurisdiction">
      <rdfs:label>sharia law jurisdiction</rdfs:label>
      <skos:definition>A Jurisdiction in which a Shari'a system of law is in force.</skos:definition>
      <rdfs:subClassOf rdf:resource="&fibo-fnd-lawx-jur;ReligiousLawJurisdiction"/>
   </owl:Class>

   <owl:Class rdf:about="&fibo-fnd-lawx-jur;ShariaLawSystem">
      <rdfs:label>sharia law system</rdfs:label>
      <skos:definition>A system of Shari'a Law.</skos:definition>
   </owl:Class>

   <owl:Class rdf:about="&fibo-fnd-lawx-jur;StatutoryLaw">
      <rdfs:label>statutory law</rdfs:label>
      <skos:definition>Written law set down by a legislature or by a legislator.</skos:definition>
   </owl:Class>


  <!--
    ///////////////////////////////////////////////////////////////////////////////////////
    //
    // Individuals
    //
    ///////////////////////////////////////////////////////////////////////////////////////
    -->


</rdf:RDF>