<?xml version="1.0" encoding="UTF-8"?>
  
<!DOCTYPE rdf:RDF [
    <!ENTITY fibo-der-ass-eqo "http://spec.edmcouncil.org/fibo/red/der/asset-derivatives/equity-options/">
    <!ENTITY fibo-fnd-agrx-cst "http://spec.edmcouncil.org/fibo/red/fnd/agreements-ext/contractual-constructs/">
    <!ENTITY fibo-der-ctr-otcd "http://spec.edmcouncil.org/fibo/red/der/derivatives-contracts/otc-derivatives/">
    <!ENTITY fibo-der-ctr-opt "http://spec.edmcouncil.org/fibo/red/der/derivatives-contracts/options/">
    <!ENTITY fibo-der-ass-ass "http://spec.edmcouncil.org/fibo/red/der/asset-derivatives/asset-derivatives/">
    <!ENTITY fibo-fnd-agr-ctr "http://spec.edmcouncil.org/fibo/red/fnd/agreements/contracts/">
    <!ENTITY fibo-fnd-law-jur "http://spec.edmcouncil.org/fibo/red/fnd/law/jurisdictions/">
    <!ENTITY fibo-fnd-acc-cur "http://spec.edmcouncil.org/fibo/red/fnd/accounting/currency-amount/">
    <!ENTITY fibo-der-ass-bas "http://spec.edmcouncil.org/fibo/red/der/asset-derivatives/asset-baskets/">
    <!ENTITY fibo-der-etd-opt "http://spec.edmcouncil.org/fibo/red/der/exchange-traded-derivatives/exchange-traded-options/">
    <!ENTITY fibo-fnd-utl-bt "http://spec.edmcouncil.org/fibo/red/fnd/utilities/business-facing-types/">
]>

<rdf:RDF xmlns:xsd="http://www.w3.org/2001/XMLSchema#"
         xmlns:sm="http://www.omg.org/techprocess/ab/SpecificationMetadata/"
         xmlns:xs="http://www.w3.org/2001/XMLSchema"
         xmlns:fibo-fnd-utl-av="http://www.omg.org/spec/EDMC-FIBO/FND/Utilities/AnnotationVocabulary/"
         xmlns:rdf="http://www.w3.org/1999/02/22-rdf-syntax-ns#"
         xmlns:rdfs="http://www.w3.org/2000/01/rdf-schema#"
         xmlns:owl="http://www.w3.org/2002/07/owl#"
         xmlns:skos="http://www.w3.org/2004/02/skos/core#"
         xmlns:dc="http://purl.org/dc/terms/"
         xml:base="http://spec.edmcouncil.org/fibo/red/der/asset-derivatives/equity-options/">

   <owl:Ontology rdf:about="http://spec.edmcouncil.org/fibo/red/der/asset-derivatives/equity-options/">
      <owl:imports rdf:resource="http://spec.edmcouncil.org/fibo/red/fnd/agreements-ext/contractual-constructs/"/>
      <owl:imports rdf:resource="http://spec.edmcouncil.org/fibo/red/der/derivatives-contracts/otc-derivatives/"/>
      <owl:imports rdf:resource="http://spec.edmcouncil.org/fibo/red/der/derivatives-contracts/options/"/>
      <owl:imports rdf:resource="http://spec.edmcouncil.org/fibo/red/der/asset-derivatives/asset-derivatives/"/>
      <owl:imports rdf:resource="http://spec.edmcouncil.org/fibo/red/fnd/agreements/contracts/"/>
      <owl:imports rdf:resource="http://spec.edmcouncil.org/fibo/red/fnd/law/jurisdictions/"/>
      <owl:imports rdf:resource="http://spec.edmcouncil.org/fibo/red/fnd/accounting/currency-amount/"/>
      <owl:imports rdf:resource="http://spec.edmcouncil.org/fibo/red/der/asset-derivatives/asset-baskets/"/>
      <owl:imports rdf:resource="http://spec.edmcouncil.org/fibo/red/der/exchange-traded-derivatives/exchange-traded-options/"/>
      <owl:imports rdf:resource="http://spec.edmcouncil.org/fibo/red/fnd/utilities/business-facing-types/"/>
   </owl:Ontology>


  <!--
    ///////////////////////////////////////////////////////////////////////////////////////
    //
    // Datatypes
    //
    ///////////////////////////////////////////////////////////////////////////////////////
    -->



  <!--
    ///////////////////////////////////////////////////////////////////////////////////////
    //
    // Object Properties
    //
    ///////////////////////////////////////////////////////////////////////////////////////
    -->


<owl:ObjectProperty rdf:about="&fibo-der-ass-eqo;hasAnnex">
      <rdfs:label>has annex</rdfs:label>
      <rdfs:subPropertyOf rdf:resource="&fibo-fnd-agr-ctr;contractHasTerms"/>
      <rdfs:domain rdf:resource="&fibo-der-ass-eqo;EquityBasketOptionOTCContract"/>
      <rdfs:range rdf:resource="&fibo-der-ass-bas;EquityBasketOptionAnnex"/>
   </owl:ObjectProperty>

   <owl:ObjectProperty rdf:about="&fibo-der-ass-eqo;underlying">
      <rdfs:label>underlying</rdfs:label>
      <rdfs:subPropertyOf rdf:resource="&fibo-der-ass-eqo;underlying.2"/>
      <rdfs:domain rdf:resource="&fibo-der-ass-eqo;EquityBasketOptionOTCContract"/>
      <rdfs:range rdf:resource="&fibo-der-ass-bas;EquityBasketObservable"/>
   </owl:ObjectProperty>

   <owl:ObjectProperty rdf:about="&fibo-der-ass-eqo;includesSpecification">
      <rdfs:label>includes specification</rdfs:label>
      <rdfs:subPropertyOf rdf:resource="&fibo-der-ctr-opt;includesSpecificationTerm"/>
      <rdfs:domain rdf:resource="&fibo-der-ass-eqo;EquityIndexOptionStrikeTermsSet"/>
      <rdfs:range rdf:resource="&fibo-der-ctr-opt;PercentageStrikePriceSpecification"/>
   </owl:ObjectProperty>

   <owl:ObjectProperty rdf:about="&fibo-der-ass-eqo;underlying.1">
      <rdfs:label>underlying</rdfs:label>
      <rdfs:subPropertyOf rdf:resource="&fibo-der-ass-eqo;underlying.2"/>
      <rdfs:domain rdf:resource="&fibo-der-ass-eqo;EquityIndexOptionOTCContract"/>
      <rdfs:range rdf:resource="&fibo-der-ass-ass;EquityIndexObservable"/>
   </owl:ObjectProperty>

   <owl:ObjectProperty rdf:about="&fibo-der-ass-eqo;embodies">
      <rdfs:label>embodies</rdfs:label>
      <rdfs:subPropertyOf rdf:resource="&fibo-der-ctr-opt;embodies"/>
      <rdfs:domain rdf:resource="&fibo-der-ass-eqo;EquityOTCOptionTransaction"/>
      <rdfs:range rdf:resource="&fibo-der-ass-eqo;EquityOptionOTCContract"/>
   </owl:ObjectProperty>

   <owl:ObjectProperty rdf:about="&fibo-der-ass-eqo;maySpecify">
      <rdfs:label>may specify</rdfs:label>
      <rdfs:domain rdf:resource="&fibo-der-ass-eqo;EquityOptionOTCContract"/>
      <rdfs:range rdf:resource="&fibo-der-etd-opt;ExchangeTradedOptionContract"/>
   </owl:ObjectProperty>

   <owl:ObjectProperty rdf:about="&fibo-der-ass-eqo;hasLocalJurisdiction">
      <rdfs:label>has local jurisdiction</rdfs:label>
      <rdfs:subPropertyOf rdf:resource="&fibo-fnd-agr-ctr;hasGoverningJurisdiction"/>
      <rdfs:domain rdf:resource="&fibo-der-ass-eqo;EquityOptionOTCContract"/>
      <rdfs:range rdf:resource="&fibo-fnd-law-jur;Jurisdiction"/>
   </owl:ObjectProperty>

   <owl:ObjectProperty rdf:about="&fibo-der-ass-eqo;hasRelevantJurisdiction">
      <rdfs:label>has relevant jurisdiction</rdfs:label>
      <rdfs:subPropertyOf rdf:resource="&fibo-fnd-agr-ctr;hasGoverningJurisdiction"/>
      <rdfs:domain rdf:resource="&fibo-der-ass-eqo;EquityOptionOTCContract"/>
      <rdfs:range rdf:resource="&fibo-fnd-law-jur;Jurisdiction"/>
   </owl:ObjectProperty>

   <owl:ObjectProperty rdf:about="&fibo-der-ass-eqo;notionalAmount">
      <rdfs:label>notional amount</rdfs:label>
      <skos:definition>'The notional amount.' Further notes: Presumably all options have a notional amount. This is defined here for Eqiuty Option. FpML: 'The notional amount.'</skos:definition>
      <rdfs:domain rdf:resource="&fibo-der-ass-eqo;EquityOptionOTCContract"/>
      <rdfs:range rdf:resource="&fibo-fnd-acc-cur;MoneyAmount"/>
   </owl:ObjectProperty>

   <owl:ObjectProperty rdf:about="&fibo-der-ass-eqo;numberOfOptions">
      <rdfs:label>number of options</rdfs:label>
      <skos:definition>The price per equity security, index or basket observed on the trade or effective date. FpML: 'The price per asset, index or basket observed on the trade or effective date.'</skos:definition>
      <rdfs:domain rdf:resource="&fibo-der-ass-eqo;EquityOptionOTCContract"/>
      <rdfs:range rdf:resource="&fibo-fnd-utl-bt;number"/>
   </owl:ObjectProperty>

   <owl:ObjectProperty rdf:about="&fibo-der-ass-eqo;underlying.2">
      <rdfs:label>underlying</rdfs:label>
      <rdfs:subPropertyOf rdf:resource="&fibo-der-ctr-opt;hasUnderlying"/>
      <rdfs:domain rdf:resource="&fibo-der-ass-eqo;EquityOptionOTCContract"/>
      <rdfs:range rdf:resource="&fibo-der-ass-ass;EquityObservable"/>
   </owl:ObjectProperty>

   <owl:ObjectProperty rdf:about="&fibo-der-ass-eqo;definesOptional">
      <rdfs:label>defines optional</rdfs:label>
      <rdfs:subPropertyOf rdf:resource="&fibo-der-ctr-opt;definesOptional.2"/>
      <rdfs:domain rdf:resource="&fibo-der-ass-eqo;EquityOptionOTCContract"/>
      <rdfs:range rdf:resource="&fibo-der-ass-eqo;EquityOTCOptionTransaction"/>
   </owl:ObjectProperty>

   <owl:ObjectProperty rdf:about="&fibo-der-ass-eqo;underlying.3">
      <rdfs:label>underlying</rdfs:label>
      <rdfs:subPropertyOf rdf:resource="&fibo-der-ass-eqo;underlying.2"/>
      <rdfs:domain rdf:resource="&fibo-der-ass-eqo;ShareOptionOTCContract"/>
      <rdfs:range rdf:resource="&fibo-der-ass-ass;SingleShareObservable"/>
   </owl:ObjectProperty>

   <owl:ObjectProperty rdf:about="&fibo-der-ass-eqo;extraordinaryEventsTreatment">
      <rdfs:label>extraordinary events treatment</rdfs:label>
      <skos:definition>Events affecting the issuer of those shares that may require the terms of the transaction to be adjusted.</skos:definition>
      <rdfs:domain rdf:resource="&fibo-der-ass-eqo;ShareOptionOTCContract"/>
      <rdfs:range rdf:resource="http://www.w3.org/2001/XMLSchema#string"/>
   </owl:ObjectProperty>

   <owl:ObjectProperty rdf:about="&fibo-der-ass-eqo;includesSpecification.1">
      <rdfs:label>includes specification</rdfs:label>
      <rdfs:subPropertyOf rdf:resource="&fibo-der-ctr-opt;includesSpecificationTerm"/>
      <rdfs:domain rdf:resource="&fibo-der-ass-eqo;ShareOptionStrikeTermsSet"/>
      <rdfs:range rdf:resource="&fibo-der-ctr-opt;AbsolutePriceStrikeSpecification"/>
   </owl:ObjectProperty>


  <!--
    ///////////////////////////////////////////////////////////////////////////////////////
    //
    // Data Properties
    //
    ///////////////////////////////////////////////////////////////////////////////////////
    -->


<owl:DatatypeProperty rdf:about="&fibo-der-ass-eqo;nearestIndexProvision">
      <rdfs:label>nearest index provision</rdfs:label>
      <skos:definition>For an index option transaction, whether the Nearest Index Contract provision is applicable.</skos:definition>
      <rdfs:range rdf:resource="&fibo-fnd-utl-bt;yesOrNo"/>
   </owl:DatatypeProperty>

   <owl:DatatypeProperty rdf:about="&fibo-der-ass-eqo;contractMultiplier">
      <rdfs:label>contract multiplier</rdfs:label>
      <skos:definition>The contract multiplier associated with the index option.</skos:definition>
      <rdfs:range rdf:resource="&fibo-fnd-utl-bt;number"/>
   </owl:DatatypeProperty>

   <owl:DatatypeProperty rdf:about="&fibo-der-ass-eqo;exchangeLookalike">
      <rdfs:label>exchange lookalike</rdfs:label>
      <skos:definition>Whether the corresponding transaction is to be treated as an 'exchange look-alike'. If Yes, then the relevant share adjustments will follow that for a corresponding designated contract listed on the related exchange</skos:definition>
      <rdfs:range rdf:resource="&fibo-fnd-utl-bt;yesOrNo"/>
   </owl:DatatypeProperty>

   <owl:DatatypeProperty rdf:about="&fibo-der-ass-eqo;novationAllowable">
      <rdfs:label>novation allowable</rdfs:label>
      <rdfs:range rdf:resource="&fibo-fnd-utl-bt;yesOrNo"/>
   </owl:DatatypeProperty>

   <owl:DatatypeProperty rdf:about="&fibo-der-ass-eqo;novationRequired">
      <rdfs:label>novation required</rdfs:label>
      <rdfs:range rdf:resource="&fibo-fnd-utl-bt;yesOrNo"/>
   </owl:DatatypeProperty>

   <owl:DatatypeProperty rdf:about="&fibo-der-ass-eqo;multiplier">
      <rdfs:label>multiplier</rdfs:label>
      <skos:definition>The contract multiplier associated with an index or basket option.</skos:definition>
      <rdfs:range rdf:resource="&fibo-fnd-utl-bt;number"/>
   </owl:DatatypeProperty>

   <owl:DatatypeProperty rdf:about="&fibo-der-ass-eqo;numberOfShares">
      <rdfs:label>number of shares</rdfs:label>
      <skos:definition>The number of shares per option comprised in the option. FpML: 'The number of shares per option comprised in the option transaction supplement.'</skos:definition>
      <rdfs:range rdf:resource="&fibo-fnd-utl-bt;number"/>
   </owl:DatatypeProperty>

   <owl:DatatypeProperty rdf:about="&fibo-der-ass-eqo;sharesPerOption">
      <rdfs:label>shares per option</rdfs:label>
      <skos:definition>The number of shares per option defined for the option contract.</skos:definition>
      <rdfs:range rdf:resource="&fibo-fnd-utl-bt;wholeNumber"/>
   </owl:DatatypeProperty>


  <!--
    ///////////////////////////////////////////////////////////////////////////////////////
    //
    // Annotation Properties
    //
    ///////////////////////////////////////////////////////////////////////////////////////
    -->



  <!--
    ///////////////////////////////////////////////////////////////////////////////////////
    //
    // Classes
    //
    ///////////////////////////////////////////////////////////////////////////////////////
    -->


<owl:Class rdf:about="&fibo-der-ass-eqo;BasketOptionStrikeTerms">
      <rdfs:label>basket option strike terms</rdfs:label>
      <skos:definition>Formal terms for the exercise of an Equity Basket Option. Further Notes Review 10 Feb: Strike price for Basket depends what is in the basket Single names: can come up with a value for the basket as a whole. Basket of Indices - would be different. Each constituent is an index. Basket that mixes single name as well as indices.</skos:definition>
      <rdfs:subClassOf rdf:resource="&fibo-der-ass-eqo;EquityOptionExerciseTermsSet"/>
   </owl:Class>

   <owl:Class rdf:about="&fibo-der-ass-eqo;EquityBasketOptionOTCContract">
      <rdfs:label>equity basket option o t c contract</rdfs:label>
      <rdfs:subClassOf rdf:resource="&fibo-der-ass-eqo;EquityOptionOTCContract"/>
   </owl:Class>

   <owl:Class rdf:about="&fibo-der-ass-eqo;EquityIndexOptionOTCContract">
      <rdfs:label>equity index option o t c contract</rdfs:label>
      <skos:definition>An option in which the underlyer is an equity index.</skos:definition>
   </owl:Class>

   <owl:Class rdf:about="&fibo-der-ass-eqo;EquityIndexOptionStrikeTermsSet">
      <rdfs:label>equity index option strike terms set</rdfs:label>
      <skos:definition>The strike price in respect of an index option transaction, is the level of the relevant index specified or otherwise determined in the transaction; This can be expressed either as a percentage of notional amount or as an absolute value.</skos:definition>
   </owl:Class>

   <owl:Class rdf:about="&fibo-der-ass-eqo;EquityOTCBasketOptionTransaction">
      <rdfs:label>equity o t c basket option transaction</rdfs:label>
      <rdfs:subClassOf rdf:resource="&fibo-der-ass-eqo;EquityOTCOptionTransaction"/>
   </owl:Class>

   <owl:Class rdf:about="&fibo-der-ass-eqo;EquityOTCOptionTransaction">
      <rdfs:label>equity o t c option transaction</rdfs:label>
      <skos:definition>A transaction which is defined in an equity options contract and which may or may not take place, at the discretion of the holder of the option. If it does take place, this will be a transaction for the purchase or sale of the equity underlying or some cash equivalent thereof, as defined in the option contract.</skos:definition>
      <rdfs:subClassOf rdf:resource="&fibo-der-ctr-opt;OptionalUnderlyingTransaction"/>
      <rdfs:subClassOf rdf:resource="&fibo-der-ctr-otcd;OTCDerivativeTransaction"/>
   </owl:Class>

   <owl:Class rdf:about="&fibo-der-ass-eqo;EquityOptionCallTransaction">
      <rdfs:label>equity option call transaction</rdfs:label>
      <skos:definition>A transaction which is defined in an equity options contract and which may or may not take place, at the discretion of the holder of the option. If it does take place, this will be a transaction for the purchase of the equity underlying or some cash equivalent thereof, as defined in the option contract.</skos:definition>
      <rdfs:subClassOf rdf:resource="&fibo-der-ctr-opt;OptionCallTransaction"/>
   </owl:Class>

   <owl:Class rdf:about="&fibo-der-ass-eqo;EquityOptionEntitlement">
      <rdfs:label>equity option entitlement</rdfs:label>
      <skos:definition>The entitlements to the holder, comprised in an option contract or transaction supplement. FpML: 'The number of shares per option comprised in the option transaction supplement.' In FpML this is an either / or: Either a whole number representing the number of shares per option, or a multiplier to be applied to an index underlyer (and, presumably, a basket underlyer)</skos:definition>
      <rdfs:subClassOf rdf:resource="&fibo-fnd-agrx-cst;ContractualRight"/>
   </owl:Class>

   <owl:Class rdf:about="&fibo-der-ass-eqo;EquityOptionExerciseTermsSet">
      <rdfs:label>equity option exercise terms set</rdfs:label>
      <skos:definition>Contractual terms setting out the price or level at which the Equity option is to be struck.</skos:definition>
      <rdfs:subClassOf rdf:resource="&fibo-der-ctr-opt;OptionExerciseTimeTermsSet"/>
   </owl:Class>

   <owl:Class rdf:about="&fibo-der-ass-eqo;EquityOptionOTCContract">
      <rdfs:label>equity option o t c contract</rdfs:label>
      <skos:definition>Definition needed</skos:definition>
      <rdfs:subClassOf rdf:resource="&fibo-der-ctr-opt;OTCOptionContract"/>
      <rdfs:subClassOf rdf:resource="&fibo-der-ass-ass;EquityDerivativeContract"/>
   </owl:Class>

   <owl:Class rdf:about="&fibo-der-ass-eqo;EquityOptionPutTransaction">
      <rdfs:label>equity option put transaction</rdfs:label>
      <skos:definition>A transaction which is defined in an equity options contract and which may or may not take place, at the discretion of the holder of the option. If it does take place, this will be a transaction for the sale of the equity underlying or some cash equivalent thereof, as defined in the option contract.</skos:definition>
      <rdfs:subClassOf rdf:resource="&fibo-der-ctr-opt;OptionPutTransaction"/>
   </owl:Class>

   <owl:Class rdf:about="&fibo-der-ass-eqo;IndexOrBasketOptionEntitlement">
      <rdfs:label>index or basket option entitlement</rdfs:label>
      <skos:definition>The entitlements to the holder of a basket or index option, comprised in an option contract or transaction supplement.</skos:definition>
      <rdfs:subClassOf rdf:resource="&fibo-der-ass-eqo;EquityOptionEntitlement"/>
   </owl:Class>

   <owl:Class rdf:about="&fibo-der-ass-eqo;ShareOptionEntitlement">
      <rdfs:label>share option entitlement</rdfs:label>
      <skos:definition>The entitlements to the holder of a single share option, comprised in an option contract or transaction supplement.</skos:definition>
   </owl:Class>

   <owl:Class rdf:about="&fibo-der-ass-eqo;ShareOptionOTCContract">
      <rdfs:label>share option o t c contract</rdfs:label>
      <skos:definition>An option in which the underlyer is a single publicly issued and traded share.</skos:definition>
   </owl:Class>

   <owl:Class rdf:about="&fibo-der-ass-eqo;ShareOptionStrikeTermsSet">
      <rdfs:label>share option strike terms set</rdfs:label>
      <skos:definition>The strike price is the price per share specified or otherwise determined in the transaction. This can be expressed either as a percentage of notional amount or as an absolute value. FpML equityStrike (complex type): A type for defining the strike price for an equity option. The strike price is either: (i) in respect of an index option transaction, the level of the relevant index specified or otherwise determined in the transaction; or (ii) in respect of a share option transaction, the price per share specified or otherwise determined in the transaction. This can be expressed either as a percentage of notional amount or as an absolute value.</skos:definition>
   </owl:Class>


  <!--
    ///////////////////////////////////////////////////////////////////////////////////////
    //
    // Individuals
    //
    ///////////////////////////////////////////////////////////////////////////////////////
    -->


</rdf:RDF>