<?xml version="1.0" encoding="UTF-8"?>
  
<!DOCTYPE rdf:RDF [
    <!ENTITY fibo-ind-mi-cri "http://spec.edmcouncil.org/fibo/red/ind/market-indices/credit-indices/">
    <!ENTITY fibo-sec-sec-bsk "http://spec.edmcouncil.org/fibo/red/sec/securities/baskets/">
    <!ENTITY fibo-ind-ind-ind "http://spec.edmcouncil.org/fibo/red/ind/indicators/indicators/">
    <!ENTITY fibo-fnd-tim-tim "http://spec.edmcouncil.org/fibo/red/fnd/date-time/date-time/">
    <!ENTITY fibo-fnd-utl-bt "http://spec.edmcouncil.org/fibo/red/fnd/utilities/business-facing-types/">
    <!ENTITY fibo-fnd-pub-pub "http://spec.edmcouncil.org/fibo/red/fnd/publications/publications/">
    <!ENTITY fibo-be-le-cb "http://spec.edmcouncil.org/fibo/red/be/legal-entities/corporate-bodies/">
    <!ENTITY fibo-sec-dbt-dbt-ins "http://spec.edmcouncil.org/fibo/red/sec/debt/debt-foundations/debt-instruments/">
    <!ENTITY fibo-md-tmp-tmp "http://spec.edmcouncil.org/fibo/red/md/temporal-core/temporal-concepts/">
    <!ENTITY fibo-md-tmp-cev "http://spec.edmcouncil.org/fibo/red/md/temporal-core/credit-events/">
    <!ENTITY fibo-fnd-acc-cur "http://spec.edmcouncil.org/fibo/red/fnd/accounting/currency-amount/">
]>

<rdf:RDF xmlns:xsd="http://www.w3.org/2001/XMLSchema#"
         xmlns:sm="http://www.omg.org/techprocess/ab/SpecificationMetadata/"
         xmlns:xs="http://www.w3.org/2001/XMLSchema"
         xmlns:fibo-fnd-utl-av="http://www.omg.org/spec/EDMC-FIBO/FND/Utilities/AnnotationVocabulary/"
         xmlns:rdf="http://www.w3.org/1999/02/22-rdf-syntax-ns#"
         xmlns:rdfs="http://www.w3.org/2000/01/rdf-schema#"
         xmlns:owl="http://www.w3.org/2002/07/owl#"
         xmlns:skos="http://www.w3.org/2004/02/skos/core#"
         xmlns:dc="http://purl.org/dc/terms/"
         xml:base="http://spec.edmcouncil.org/fibo/red/ind/market-indices/credit-indices/">

   <owl:Ontology rdf:about="http://spec.edmcouncil.org/fibo/red/ind/market-indices/credit-indices/">
      <owl:imports rdf:resource="http://spec.edmcouncil.org/fibo/red/sec/securities/baskets/"/>
      <owl:imports rdf:resource="http://spec.edmcouncil.org/fibo/red/ind/indicators/indicators/"/>
      <owl:imports rdf:resource="http://spec.edmcouncil.org/fibo/red/fnd/date-time/date-time/"/>
      <owl:imports rdf:resource="http://spec.edmcouncil.org/fibo/red/fnd/utilities/business-facing-types/"/>
      <owl:imports rdf:resource="http://spec.edmcouncil.org/fibo/red/fnd/publications/publications/"/>
      <owl:imports rdf:resource="http://spec.edmcouncil.org/fibo/red/be/legal-entities/corporate-bodies/"/>
      <owl:imports rdf:resource="http://spec.edmcouncil.org/fibo/red/sec/debt/debt-foundations/debt-instruments/"/>
      <owl:imports rdf:resource="http://spec.edmcouncil.org/fibo/red/md/temporal-core/temporal-concepts/"/>
      <owl:imports rdf:resource="http://spec.edmcouncil.org/fibo/red/md/temporal-core/credit-events/"/>
      <owl:imports rdf:resource="http://spec.edmcouncil.org/fibo/red/fnd/accounting/currency-amount/"/>
   </owl:Ontology>


  <!--
    ///////////////////////////////////////////////////////////////////////////////////////
    //
    // Datatypes
    //
    ///////////////////////////////////////////////////////////////////////////////////////
    -->



  <!--
    ///////////////////////////////////////////////////////////////////////////////////////
    //
    // Object Properties
    //
    ///////////////////////////////////////////////////////////////////////////////////////
    -->


<owl:ObjectProperty rdf:about="&fibo-ind-mi-cri;hasConstituent">
      <rdfs:label>has constituent</rdfs:label>
      <rdfs:subPropertyOf rdf:resource="&fibo-sec-sec-bsk;hasConstituent.2"/>
      <rdfs:domain rdf:resource="&fibo-ind-mi-cri;BasketOfCreditRisks"/>
      <rdfs:range rdf:resource="&fibo-ind-mi-cri;CreditIndexReferenceConstituent"/>
   </owl:ObjectProperty>

   <owl:ObjectProperty rdf:about="&fibo-ind-mi-cri;currentNotionalValue">
      <rdfs:label>current notional value</rdfs:label>
      <skos:definition>The notional amount of the index at the present time or at a defined point in the past.</skos:definition>
      <rdfs:domain rdf:resource="&fibo-ind-mi-cri;CreditIndex"/>
      <rdfs:range rdf:resource="&fibo-md-tmp-tmp;DatedMonetaryAmount"/>
   </owl:ObjectProperty>

   <owl:ObjectProperty rdf:about="&fibo-ind-mi-cri;maturity">
      <rdfs:label>maturity</rdfs:label>
      <skos:definition>The maturity of protection represented by the index as a length of time (dated duration specification).</skos:definition>
      <rdfs:domain rdf:resource="&fibo-ind-mi-cri;CreditIndex"/>
      <rdfs:range rdf:resource="&fibo-fnd-tim-tim;KnownDateDuration"/>
   </owl:ObjectProperty>

   <owl:ObjectProperty rdf:about="&fibo-ind-mi-cri;originalNotional">
      <rdfs:label>original notional</rdfs:label>
      <skos:definition>The notional amount represented by the index when it is first constituted.</skos:definition>
      <rdfs:domain rdf:resource="&fibo-ind-mi-cri;CreditIndex"/>
      <rdfs:range rdf:resource="&fibo-fnd-acc-cur;MonetaryAmount"/>
   </owl:ObjectProperty>

   <owl:ObjectProperty rdf:about="&fibo-ind-mi-cri;premium">
      <rdfs:label>premium</rdfs:label>
      <skos:definition>A premium payable for a contract based on the index.</skos:definition>
      <rdfs:domain rdf:resource="&fibo-ind-mi-cri;CreditIndex"/>
      <rdfs:range rdf:resource="&fibo-fnd-acc-cur;MonetaryAmount"/>
   </owl:ObjectProperty>

   <owl:ObjectProperty rdf:about="&fibo-ind-mi-cri;upFrontFee">
      <rdfs:label>up front fee</rdfs:label>
      <skos:definition>A fee payanle by any party that wishes to participate in a contract based on the index after the start of its life.</skos:definition>
      <rdfs:domain rdf:resource="&fibo-ind-mi-cri;CreditIndex"/>
      <rdfs:range rdf:resource="&fibo-fnd-acc-cur;MonetaryAmount"/>
   </owl:ObjectProperty>

   <owl:ObjectProperty rdf:about="&fibo-ind-mi-cri;currency">
      <rdfs:label>currency</rdfs:label>
      <skos:definition>The currency in which the reference instrument is denominated.</skos:definition>
      <rdfs:domain rdf:resource="&fibo-ind-mi-cri;CreditIndexReferenceConstituent"/>
      <rdfs:range rdf:resource="&fibo-fnd-utl-bt;text"/>
   </owl:ObjectProperty>

   <owl:ObjectProperty rdf:about="&fibo-ind-mi-cri;debtRanking">
      <rdfs:label>debt ranking</rdfs:label>
      <skos:definition>An indication of the ranking of this debt.</skos:definition>
      <rdfs:domain rdf:resource="&fibo-ind-mi-cri;CreditIndexReferenceConstituent"/>
      <rdfs:range rdf:resource="http://www.w3.org/2001/XMLSchema#string"/>
   </owl:ObjectProperty>

   <owl:ObjectProperty rdf:about="&fibo-ind-mi-cri;maturity.1">
      <rdfs:label>maturity</rdfs:label>
      <skos:definition>The maturity of the instrument, specified as a length of time (dated duration specification). This is a specified duration, denominated in calendar units.</skos:definition>
      <rdfs:domain rdf:resource="&fibo-ind-mi-cri;CreditIndexReferenceConstituent"/>
      <rdfs:range rdf:resource="&fibo-md-tmp-tmp;DatedDurationSpecification"/>
   </owl:ObjectProperty>

   <owl:ObjectProperty rdf:about="&fibo-ind-mi-cri;isConstituentOf">
      <rdfs:label>is constituent of</rdfs:label>
      <rdfs:domain rdf:resource="&fibo-ind-mi-cri;CreditIndexReferenceConstituent"/>
      <rdfs:range rdf:resource="&fibo-ind-mi-cri;BasketOfCreditRisks"/>
      <owl:inverseOf rdf:resource="&fibo-ind-mi-cri;hasConstituent"/>
   </owl:ObjectProperty>

   <owl:ObjectProperty rdf:about="&fibo-ind-mi-cri;referenceEntityIdentity">
      <rdfs:label>reference entity identity</rdfs:label>
      <rdfs:subPropertyOf rdf:resource="&fibo-sec-sec-bsk;identity"/>
      <rdfs:domain rdf:resource="&fibo-ind-mi-cri;CreditIndexReferenceConstituent"/>
      <rdfs:range rdf:resource="&fibo-be-le-cb;BodyCorporate"/>
   </owl:ObjectProperty>

   <owl:ObjectProperty rdf:about="&fibo-ind-mi-cri;referenceSecurityIdentity">
      <rdfs:label>reference security identity</rdfs:label>
      <rdfs:subPropertyOf rdf:resource="&fibo-sec-sec-bsk;identity"/>
      <rdfs:domain rdf:resource="&fibo-ind-mi-cri;CreditIndexReferenceConstituent"/>
      <rdfs:range rdf:resource="&fibo-sec-dbt-dbt-ins;TradableDebtInstrument"/>
   </owl:ObjectProperty>

   <owl:ObjectProperty rdf:about="&fibo-ind-mi-cri;refersTo">
      <rdfs:label>refers to</rdfs:label>
      <rdfs:subPropertyOf rdf:resource="&fibo-fnd-pub-pub;isAbout"/>
      <rdfs:domain rdf:resource="&fibo-ind-mi-cri;CreditIndexReferenceConstituent"/>
      <rdfs:range rdf:resource="&fibo-md-tmp-cev;CreditEvent"/>
   </owl:ObjectProperty>

   <owl:ObjectProperty rdf:about="&fibo-ind-mi-cri;representsRiskOf">
      <rdfs:label>represents risk of</rdfs:label>
      <rdfs:subPropertyOf rdf:resource="&fibo-fnd-pub-pub;isAbout"/>
      <rdfs:domain rdf:resource="&fibo-ind-mi-cri;CreditIndex"/>
      <rdfs:range rdf:resource="&fibo-ind-mi-cri;BasketOfCreditRisks"/>
   </owl:ObjectProperty>


  <!--
    ///////////////////////////////////////////////////////////////////////////////////////
    //
    // Data Properties
    //
    ///////////////////////////////////////////////////////////////////////////////////////
    -->


<owl:DatatypeProperty rdf:about="&fibo-ind-mi-cri;assetType">
      <rdfs:label>asset type</rdfs:label>
      <skos:definition>The types of asset which make up the index. Further notes: There is a variety of indices build around different common creiteria, of which this is one. Variety: asset type (loan, bond, mortgage-backed, asset-backed).</skos:definition>
      <rdfs:range rdf:resource="&fibo-fnd-utl-bt;text"/>
   </owl:DatatypeProperty>

   <owl:DatatypeProperty rdf:about="&fibo-ind-mi-cri;indexName">
      <rdfs:label>index name</rdfs:label>
      <skos:definition>The formal name of the index.</skos:definition>
      <rdfs:range rdf:resource="&fibo-fnd-utl-bt;text"/>
   </owl:DatatypeProperty>

   <owl:DatatypeProperty rdf:about="&fibo-ind-mi-cri;sector">
      <rdfs:label>sector</rdfs:label>
      <skos:definition>The sector from which constituents of the index are all drawn.</skos:definition>
      <rdfs:range rdf:resource="&fibo-fnd-utl-bt;text"/>
   </owl:DatatypeProperty>

   <owl:DatatypeProperty rdf:about="&fibo-ind-mi-cri;spreadRange">
      <rdfs:label>spread range</rdfs:label>
      <skos:definition>The range of credit spread for the constituents of the index.</skos:definition>
      <rdfs:range rdf:resource="&fibo-fnd-utl-bt;text"/>
   </owl:DatatypeProperty>

   <owl:DatatypeProperty rdf:about="&fibo-ind-mi-cri;indexConstituentID">
      <rdfs:label>index constituent i d</rdfs:label>
      <skos:definition>An identifier for this constituent of this index, published by the index provider. Further notes: Example: Markit REDCODE reference entity ID</skos:definition>
      <rdfs:range rdf:resource="&fibo-fnd-utl-bt;text"/>
   </owl:DatatypeProperty>

   <owl:DatatypeProperty rdf:about="&fibo-ind-mi-cri;tCM">
      <rdfs:label>t c m</rdfs:label>
      <skos:definition>Description of the reference instrument in TCM format (ticker-coupon-maturity).</skos:definition>
      <rdfs:range rdf:resource="&fibo-fnd-utl-bt;text"/>
   </owl:DatatypeProperty>

   <owl:DatatypeProperty rdf:about="&fibo-ind-mi-cri;ticker">
      <rdfs:label>ticker</rdfs:label>
      <skos:definition>A local ticker identifier for the index constituent.</skos:definition>
      <rdfs:range rdf:resource="&fibo-fnd-utl-bt;text"/>
   </owl:DatatypeProperty>

   <owl:DatatypeProperty rdf:about="&fibo-ind-mi-cri;weight">
      <rdfs:label>weight</rdfs:label>
      <skos:definition>The percentage weight of this constituent in relation to the index as a whole.</skos:definition>
      <rdfs:range rdf:resource="&fibo-fnd-utl-bt;percentage"/>
   </owl:DatatypeProperty>


  <!--
    ///////////////////////////////////////////////////////////////////////////////////////
    //
    // Annotation Properties
    //
    ///////////////////////////////////////////////////////////////////////////////////////
    -->



  <!--
    ///////////////////////////////////////////////////////////////////////////////////////
    //
    // Classes
    //
    ///////////////////////////////////////////////////////////////////////////////////////
    -->


<owl:Class rdf:about="&fibo-ind-mi-cri;BasketOfCreditRisks">
      <rdfs:label>basket of credit risks</rdfs:label>
      <skos:definition>A basket of securities and / or legal entities, collected for the purpose of identifying risk.</skos:definition>
      <rdfs:subClassOf rdf:resource="&fibo-sec-sec-bsk;Basket"/>
   </owl:Class>

   <owl:Class rdf:about="&fibo-ind-mi-cri;CreditIndex">
      <rdfs:label>credit index</rdfs:label>
      <skos:definition>An index that is a function of credit events. These are Credit events occurring that change the value of an underlying portfolio.</skos:definition>
      <rdfs:subClassOf rdf:resource="&fibo-ind-ind-ind;MarketReferentialParameter"/>
   </owl:Class>

   <owl:Class rdf:about="&fibo-ind-mi-cri;CreditIndexReferenceConstituent">
      <rdfs:label>credit index reference constituent</rdfs:label>
      <skos:definition>A constituent of a basket of credit risks, such as that used in a credit index.</skos:definition>
      <rdfs:subClassOf rdf:resource="&fibo-sec-sec-bsk;BasketConstituent"/>
   </owl:Class>


  <!--
    ///////////////////////////////////////////////////////////////////////////////////////
    //
    // Individuals
    //
    ///////////////////////////////////////////////////////////////////////////////////////
    -->


</rdf:RDF>