<?xml version="1.0" encoding="UTF-8"?>
<!DOCTYPE rdf:RDF [
	<!ENTITY fibo-fnd-acc-cur "https://spec.edmcouncil.org/fibo/FND/Accounting/CurrencyAmount/">
	<!ENTITY fibo-fnd-agr-ctr "https://spec.edmcouncil.org/fibo/FND/Agreements/Contracts/">
	<!ENTITY fibo-fnd-rel-rel "https://spec.edmcouncil.org/fibo/FND/Relations/Relations/">
	<!ENTITY fibo-fnd-tim-tim "https://spec.edmcouncil.org/fibo/FND/Time/Time/">
	<!ENTITY fibo-fnd-utl-av "https://spec.edmcouncil.org/fibo/FND/Utilities/AnnotationVocabulary/">
	<!ENTITY fibo-fnd-utl-val "https://spec.edmcouncil.org/fibo/FND/Utilities/Values/">
	<!ENTITY fibo-sec-dbt-mm-td "https://spec.edmcouncil.org/fibo/SEC/Debt/MoneyMarkets/TermDeposits/">
	<!ENTITY owl "http://www.w3.org/2002/07/owl#">
	<!ENTITY rdf "http://www.w3.org/1999/02/22-rdf-syntax-ns#">
	<!ENTITY rdfs "http://www.w3.org/2000/01/rdf-schema#">
	<!ENTITY skos "http://www.w3.org/2004/02/skos/core#">
	<!ENTITY xsd "http://www.w3.org/2001/XMLSchema#">
]>
<rdf:RDF xml:base="https://spec.edmcouncil.org/fibo/SEC/Debt/MoneyMarkets/TermDeposits/"
	xmlns:fibo-fnd-acc-cur="https://spec.edmcouncil.org/fibo/FND/Accounting/CurrencyAmount/"
	xmlns:fibo-fnd-agr-ctr="https://spec.edmcouncil.org/fibo/FND/Agreements/Contracts/"
	xmlns:fibo-fnd-rel-rel="https://spec.edmcouncil.org/fibo/FND/Relations/Relations/"
	xmlns:fibo-fnd-tim-tim="https://spec.edmcouncil.org/fibo/FND/Time/Time/"
	xmlns:fibo-fnd-utl-av="https://spec.edmcouncil.org/fibo/FND/Utilities/AnnotationVocabulary/"
	xmlns:fibo-fnd-utl-val="https://spec.edmcouncil.org/fibo/FND/Utilities/Values/"
	xmlns:fibo-sec-dbt-mm-td="https://spec.edmcouncil.org/fibo/SEC/Debt/MoneyMarkets/TermDeposits/"
	xmlns:owl="http://www.w3.org/2002/07/owl#"
	xmlns:rdf="http://www.w3.org/1999/02/22-rdf-syntax-ns#"
	xmlns:rdfs="http://www.w3.org/2000/01/rdf-schema#"
	xmlns:skos="http://www.w3.org/2004/02/skos/core#"
	xmlns:xsd="http://www.w3.org/2001/XMLSchema#">
	
	<owl:Ontology rdf:about="https://spec.edmcouncil.org/fibo/SEC/Debt/MoneyMarkets/TermDeposits/">
		<rdfs:label xml:lang="en">TermDeposits</rdfs:label>
		<owl:imports rdf:resource="http://www.w3.org/2004/02/skos/core"/>
		<owl:imports rdf:resource="https://spec.edmcouncil.org/fibo/DER/DerivativesContracts/OTCInstruments/"/>
		<owl:imports rdf:resource="https://spec.edmcouncil.org/fibo/FND/Accounting/CurrencyAmount/"/>
		<owl:imports rdf:resource="https://spec.edmcouncil.org/fibo/FND/Agreements/Contracts/"/>
		<owl:imports rdf:resource="https://spec.edmcouncil.org/fibo/FND/Relations/Relations/"/>
		<owl:imports rdf:resource="https://spec.edmcouncil.org/fibo/FND/Time/Time/"/>
		<owl:imports rdf:resource="https://spec.edmcouncil.org/fibo/FND/Utilities/AnnotationVocabulary/"/>
		<owl:imports rdf:resource="https://spec.edmcouncil.org/fibo/FND/Utilities/Values/"/>
	</owl:Ontology>
	
	<owl:Class rdf:about="&fibo-sec-dbt-mm-td;TermDeposit">
		<rdfs:subClassOf rdf:resource="https://spec.edmcouncil.org/fibo/DER/DerivativesContracts/OTCInstruments/OTCInstrument"/>
		<rdfs:subClassOf>
			<owl:Restriction>
				<owl:onProperty rdf:resource="&fibo-sec-dbt-mm-td;settlementTerms"/>
				<owl:someValuesFrom rdf:resource="&fibo-sec-dbt-mm-td;TermDepositSettlementTerms"/>
			</owl:Restriction>
		</rdfs:subClassOf>
		<rdfs:label xml:lang="en">term deposit</rdfs:label>
		<skos:definition xml:lang="en">A money deposit at a bank that cannot be withdrawn for a certain &quot;term&quot; or period of time. When the term is over it can be withdrawn or it can be held for another term. The longer the term the better the yield on the money. A certificate of deposit is a time deposit product.</skos:definition>
	</owl:Class>
	
	<owl:Class rdf:about="&fibo-sec-dbt-mm-td;TermDepositSettlementTerms">
		<rdfs:subClassOf rdf:resource="https://spec.edmcouncil.org/fibo/DER/DerivativesContracts/OTCInstruments/OTCContractSettlementTerms"/>
		<rdfs:label xml:lang="en">term deposit settlement terms</rdfs:label>
		<skos:definition xml:lang="en">Contractual terms for the settlement of a Term Deposit.</skos:definition>
	</owl:Class>
	
	<owl:ObjectProperty rdf:about="&fibo-sec-dbt-mm-td;amount">
		<rdfs:label xml:lang="en">amount</rdfs:label>
		<rdfs:domain rdf:resource="&fibo-sec-dbt-mm-td;TermDeposit"/>
		<rdfs:range rdf:resource="&fibo-fnd-acc-cur;MonetaryAmount"/>
		<skos:definition xml:lang="en">The principal amount deposited.</skos:definition>
	</owl:ObjectProperty>
	
	<owl:ObjectProperty rdf:about="&fibo-sec-dbt-mm-td;settlementTerms">
		<rdfs:subPropertyOf rdf:resource="&fibo-fnd-agr-ctr;hasContractualElement"/>
		<rdfs:label xml:lang="en">settlement terms</rdfs:label>
		<rdfs:domain rdf:resource="&fibo-sec-dbt-mm-td;TermDeposit"/>
		<rdfs:range rdf:resource="&fibo-sec-dbt-mm-td;TermDepositSettlementTerms"/>
		<skos:definition xml:lang="en">The contractual terms specifying the obligations of the certificate holder for the specified duration of that deposit.</skos:definition>
	</owl:ObjectProperty>
	
	<owl:ObjectProperty rdf:about="&fibo-sec-dbt-mm-td;termDepositRate">
		<rdfs:label xml:lang="en">term deposit rate</rdfs:label>
		<rdfs:domain rdf:resource="&fibo-sec-dbt-mm-td;TermDeposit"/>
		<rdfs:range rdf:resource="&fibo-fnd-utl-val;PercentageValue"/>
		<skos:definition xml:lang="en">The rate of return on the deposit.</skos:definition>
	</owl:ObjectProperty>
	
	<owl:ObjectProperty rdf:about="&fibo-sec-dbt-mm-td;termDuration">
		<rdfs:label xml:lang="en">term duration</rdfs:label>
		<rdfs:domain rdf:resource="&fibo-sec-dbt-mm-td;TermDeposit"/>
		<rdfs:range rdf:resource="&fibo-fnd-tim-tim;Duration"/>
		<skos:definition xml:lang="en">The duration of the term specified in days, months, quarters or years.</skos:definition>
	</owl:ObjectProperty>

</rdf:RDF>