<?xml version="1.0"?>
<rdf:RDF
    xmlns:skos="http://www.w3.org/2004/02/skos/core#"
    xmlns:fibo-fnd-org-fm="http://www.omg.org/spec/EDMC-FIBO/FND/Organizations/FormalOrganizations/"
    xmlns:fibo-fnd-plc-loc="http://www.omg.org/spec/EDMC-FIBO/FND/Places/Locations/"
    xmlns:fibo-fnd-aap-ppl="http://www.omg.org/spec/EDMC-FIBO/FND/AgentsAndPeople/People/"
    xmlns:fibo-fnd-rel-rel="http://www.omg.org/spec/EDMC-FIBO/FND/Relations/Relations/"
    xmlns:fibo-fnd-plc-cty="http://www.omg.org/spec/EDMC-FIBO/FND/Places/Countries/"
    xmlns:fibo-fnd-law-cor="http://www.omg.org/spec/EDMC-FIBO/FND/Law/LegalCore/"
    xmlns:fibo-fnd-law-jur="http://www.omg.org/spec/EDMC-FIBO/FND/Law/Jurisdiction/"
    xmlns:fibo-fnd-plc-adr="http://www.omg.org/spec/EDMC-FIBO/FND/Places/Addresses/"
    xmlns:fibo-fnd-gao-gl="http://www.omg.org/spec/EDMC-FIBO/FND/GoalsAndObjectives/Goals/"
    xmlns:sm="http://www.omg.org/techprocess/ab/SpecificationMetadata/"
    xmlns:fibo-fnd-utl-av="http://www.omg.org/spec/EDMC-FIBO/FND/Utilities/AnnotationVocabulary/"
    xmlns:rdf="http://www.w3.org/1999/02/22-rdf-syntax-ns#"
    xmlns:fibo-fnd-utl-bt="http://www.omg.org/spec/EDMC-FIBO/FND/Utilities/BusinessFacingTypes/"
    xmlns:fibo-fnd-pty-rl="http://www.omg.org/spec/EDMC-FIBO/FND/Parties/Roles/"
    xmlns:owl="http://www.w3.org/2002/07/owl#"
    xmlns:fibo-fnd-org-org="http://www.omg.org/spec/EDMC-FIBO/FND/Organizations/Organizations/"
    xmlns:dct="http://purl.org/dc/terms/"
    xmlns:fibo-fnd-aap-agt="http://www.omg.org/spec/EDMC-FIBO/FND/AgentsAndPeople/Agents/"
    xmlns:xsd="http://www.w3.org/2001/XMLSchema#"
    xmlns:fibo-fnd-pty-pty="http://www.omg.org/spec/EDMC-FIBO/FND/Parties/Parties/"
    xmlns:fibo-fnd-agr-agr="http://www.omg.org/spec/EDMC-FIBO/FND/Agreements/Agreements/"
    xmlns:fibo-fnd-agr-ctr="http://www.omg.org/spec/EDMC-FIBO/FND/Agreements/Contracts/"
    xmlns:rdfs="http://www.w3.org/2000/01/rdf-schema#"
  xml:base="http://www.omg.org/spec/EDMC-FIBO/FND/Agreements/Contracts/">
  <owl:Ontology rdf:about="">
    <sm:fileAbbreviation rdf:datatype="http://www.w3.org/2001/XMLSchema#string"
    >fibo-fnd-agr-ctr</sm:fileAbbreviation>
    <sm:priorVersion rdf:datatype="http://www.w3.org/2001/XMLSchema#anyURI"
    >http://www.omg.org/spec/FIBO/Foundations/20130601/Agreements/Contracts.owl</sm:priorVersion>
    <sm:dependsOn rdf:datatype="http://www.w3.org/2001/XMLSchema#anyURI"
    >http://www.omg.org/spec/EDMC-FIBO/FND/AgentsAndPeople/Agents/</sm:dependsOn>
    <sm:filename rdf:datatype="http://www.w3.org/2001/XMLSchema#string"
    >Contracts Ontology</sm:filename>
    <rdfs:label>Financial Industry Business Ontology (FIBO) Contracts Ontology</rdfs:label>
    <sm:dependsOn rdf:datatype="http://www.w3.org/2001/XMLSchema#anyURI"
    >http://www.omg.org/spec/EDMC-FIBO/FND/Organizations/FormalOrganizations/</sm:dependsOn>
    <sm:moduleName rdf:datatype="http://www.w3.org/2001/XMLSchema#string"
    >Agreements </sm:moduleName>
    <sm:thisVersion rdf:datatype="http://www.w3.org/2001/XMLSchema#string"
    >1.0 </sm:thisVersion>
    <sm:familyURL rdf:datatype="http://www.w3.org/2001/XMLSchema#anyURI"
    >http://www.omg.org/spec/EDMC-FIBO/</sm:familyURL>
    <sm:dependsOn rdf:datatype="http://www.w3.org/2001/XMLSchema#anyURI"
    >http://www.omg.org/spec/EDMC-FIBO/FND/AgentsAndPeople/People/</sm:dependsOn>
    <sm:dependsOn rdf:datatype="http://www.w3.org/2001/XMLSchema#anyURI"
    >http://www.omg.org/spec/EDMC-FIBO/FND/Utilities/AnnotationVocabulary/</sm:dependsOn>
    <sm:keyword rdf:datatype="http://www.w3.org/2001/XMLSchema#string"
    >foundational vocabulary</sm:keyword>
    <sm:dependsOn rdf:datatype="http://www.w3.org/2001/XMLSchema#anyURI"
    >http://www.omg.org/spec/EDMC-FIBO/FND/Parties/Parties/</sm:dependsOn>
    <sm:dependsOn rdf:datatype="http://www.w3.org/2001/XMLSchema#anyURI"
    >http://www.omg.org/spec/EDMC-FIBO/FND/Parties/Roles/</sm:dependsOn>
    <sm:dependsOn rdf:datatype="http://www.w3.org/2001/XMLSchema#anyURI"
    >http://www.omg.org/spec/EDMC-FIBO/FND/Places/Addresses/</sm:dependsOn>
    <sm:dependsOn rdf:datatype="http://www.w3.org/2001/XMLSchema#anyURI"
    >http://www.omg.org/techprocess/ab/SpecificationMetadata/</sm:dependsOn>
    <sm:responsibleTaskForce rdf:datatype="http://www.w3.org/2001/XMLSchema#anyURI"
    >http://fdtf.omg.org/</sm:responsibleTaskForce>
    <sm:familyAbstract rdf:datatype="http://www.w3.org/2001/XMLSchema#string"
    >The content that comprises the Financial Industry Business Ontology (FIBO) is documentation, interpretable in formal logic, of the concepts represented by finance industry terms as used in official financial organization documents such as contracts, product/service specifications and governance and regulatory compliance documents.</sm:familyAbstract>
    <sm:keyword rdf:datatype="http://www.w3.org/2001/XMLSchema#string"
    >ontology</sm:keyword>
    <sm:dependsOn rdf:datatype="http://www.w3.org/2001/XMLSchema#anyURI"
    >http://www.omg.org/spec/EDMC-FIBO/FND/Law/Jurisdiction/</sm:dependsOn>
    <sm:moduleAbbreviation rdf:datatype="http://www.w3.org/2001/XMLSchema#string"
    >FIBO-FND-AGR</sm:moduleAbbreviation>
    <sm:contentLanguage rdf:datatype="http://www.w3.org/2001/XMLSchema#anyURI"
    >http://www.w3.org/standards/techs/owl#w3c_all</sm:contentLanguage>
    <sm:dependsOn rdf:datatype="http://www.w3.org/2001/XMLSchema#anyURI"
    >http://www.omg.org/spec/EDMC-FIBO/FND/Places/Countries/</sm:dependsOn>
    <sm:familyAbbreviation rdf:datatype="http://www.w3.org/2001/XMLSchema#string"
    >FIBO</sm:familyAbbreviation>
    <sm:moduleVersion rdf:datatype="http://www.w3.org/2001/XMLSchema#string"
    >1.0</sm:moduleVersion>
    <sm:keyword rdf:datatype="http://www.w3.org/2001/XMLSchema#string"
    >vocabulary</sm:keyword>
    <sm:technologyArea rdf:datatype="http://www.w3.org/2001/XMLSchema#string"
    >formal semantics</sm:technologyArea>
    <sm:dependsOn rdf:datatype="http://www.w3.org/2001/XMLSchema#anyURI"
    >http://www.omg.org/spec/EDMC-FIBO/FND/Places/Locations/</sm:dependsOn>
    <sm:specificationAbbreviation rdf:datatype="http://www.w3.org/2001/XMLSchema#string"
    >FIBO-FND</sm:specificationAbbreviation>
    <sm:keyword rdf:datatype="http://www.w3.org/2001/XMLSchema#string"
    >Financial Industry Business Ontology</sm:keyword>
    <sm:fileAbstract rdf:datatype="http://www.w3.org/2001/XMLSchema#string"
    >This ontology defines concepts relating to contracts, for use in other FIBO ontology elements. These include written contracts which are the concrete evidence of agreements between parties, along with verbal contracts. Contracts are further broken down into bilateral and transferable contracts, the latter being the basis for most financial instruments. Properties of contracts are also defined, in particular contractual terms and contract parties. These concepts all form the basis of concepts in the financial services industry, for example interest payment terms are a kind of contract terms set, and security holders are a kind of contract counterparty.</sm:fileAbstract>
    <owl:versionIRI rdf:datatype="http://www.w3.org/2001/XMLSchema#anyURI"
    >http://www.omg.org/spec/EDMC-FIBO/FND/20130801/Agreements/Contracts/</owl:versionIRI>
    <sm:specificationAbstract rdf:datatype="http://www.w3.org/2001/XMLSchema#string"
    >FIBO Foundations is a set of business concepts which are intended to support the financial industry terms semantics presented in other FIBO specifications.  

The FIBO Foundations models define concepts which are not unique to the financial services industry. From these, financial industry terms in other FIBO specifications may be derived by extension. Terms are also included which may be referred to by properties of things in those specifications. FIBO Foundations therefore includes a number of basic terms about legal, contractual and organizational concepts, among others. </sm:specificationAbstract>
    <sm:moduleAbstract rdf:datatype="http://www.w3.org/2001/XMLSchema#string"
    >This module includes ontologies describing agreements between parties and contracts that formalize those agreements.  These cover written and verbal contracts, including contracts which may be transferred from one party to another. The latter form the basis for financial securities contracts.  The Contracts ontology also describes fundamental properties of contracts such as contractual terms, contract parties and so on, many of which form the basis for more specialized financial industry concepts such as interest payment terms, bond issuers and so on.</sm:moduleAbstract>
    <sm:contributor rdf:datatype="http://www.w3.org/2001/XMLSchema#string"
    >Thematix Partners LLC</sm:contributor>
    <sm:dependsOn rdf:datatype="http://www.w3.org/2001/XMLSchema#anyURI"
    >http://www.omg.org/spec/EDMC-FIBO/FND/Organizations/Organizations/</sm:dependsOn>
    <sm:copyright rdf:datatype="http://www.w3.org/2001/XMLSchema#string"
    >Copyright (c) 2013 EDM Council, Inc.
Copyright (c) 2013 Object Management Group, Inc.</sm:copyright>
    <sm:specificationVersionURL rdf:datatype="http://www.w3.org/2001/XMLSchema#anyURI"
    >http://www.omg.org/spec/EDMC-FIBO/FND/1.0/</sm:specificationVersionURL>
    <skos:historyNote rdf:datatype="http://www.w3.org/2001/XMLSchema#string"
    >This version of the FIBO Foundations Specification was revised primarily to reflect comments received at the March 2013 OMG Technical Meeting in Reston and reflected in the Errata discussed at the June 2013 OMG Technical Meeting in Berlin. 

Revisions to FIBO Foundations are managed per the process outlined in the Policies and Procedures for OMG standards, with the intent to maintain backwards compatibility in the ontologies to the degree possible.
  
The RDF/XML serialized OWL for the Foundations ODM/OWL ontologies have been checked for syntactic errors and logical consistency with Protege 4 (http://protege.stanford.edu/), HermiT 1.3.7 (http://www.hermit-reasoner.com/) and Pellet 2.2 (http://clarkparsia.com/pellet/).</skos:historyNote>
    <skos:changeNote rdf:datatype="http://www.w3.org/2001/XMLSchema#string"
    >This version of the ontology was revised in advance of the September 2013 New Brunswick, NJ meeting, as follows:
   (1) to use slash style URI/IRIss (also called 303 URIs, vs. hash style) as required to support server side processing 
   (2) to use version-independent IRIs for all definitions internally as opposed to version-specific IRIs
   (3) to change the file suffix from .owl to .rdf to increase usability in RDF tools
   (4) to use 4-level abbreviations and corresponding namespace prefixes for all FIBO ontologies, reflecting a family/specification/module/ontology structure
   (5) to incorporate changes to the specification metadata to support documentation at the family, specification, module, and ontology level, similar to the abbreviations.</skos:changeNote>
    <sm:submitter rdf:datatype="http://www.w3.org/2001/XMLSchema#string"
    >EDM Council, Inc.</sm:submitter>
    <sm:contentLanguage rdf:datatype="http://www.w3.org/2001/XMLSchema#anyURI"
    >http://www.omg.org/spec/ODM/</sm:contentLanguage>
    <sm:specificationVersionStatus rdf:datatype="http://www.w3.org/2001/XMLSchema#string"
    >Request For Comments (RFC)</sm:specificationVersionStatus>
    <sm:dependsOn rdf:datatype="http://www.w3.org/2001/XMLSchema#anyURI"
    >http://www.omg.org/spec/EDMC-FIBO/FND/Law/LegalCore/</sm:dependsOn>
    <sm:keyword rdf:datatype="http://www.w3.org/2001/XMLSchema#string"
    >FIBO</sm:keyword>
    <sm:addressForComments rdf:datatype="http://www.w3.org/2001/XMLSchema#anyURI"
    >http://www.omg.org/issues/</sm:addressForComments>
    <sm:familyTitle rdf:datatype="http://www.w3.org/2001/XMLSchema#string"
    >Financial Industry Business Ontology (FIBO)</sm:familyTitle>
    <owl:imports rdf:resource="http://www.omg.org/spec/EDMC-FIBO/FND/Law/Jurisdiction/"/>
    <sm:specificationTitle rdf:datatype="http://www.w3.org/2001/XMLSchema#string"
    >Financial Industry Business Ontology (FIBO) Foundations Specification</sm:specificationTitle>
    <sm:dependsOn rdf:datatype="http://www.w3.org/2001/XMLSchema#anyURI"
    >http://www.omg.org/spec/EDMC-FIBO/FND/GoalsAndObjectives/Goals/</sm:dependsOn>
    <sm:dependsOn rdf:datatype="http://www.w3.org/2001/XMLSchema#anyURI"
    >http://www.omg.org/spec/EDMC-FIBO/FND/Utilities/BusinessFacingTypes/</sm:dependsOn>
    <sm:contributor rdf:datatype="http://www.w3.org/2001/XMLSchema#string"
    >Adaptive, Inc.</sm:contributor>
    <sm:publicationDate rdf:datatype="http://www.w3.org/2001/XMLSchema#dateTime"
    >2013-08-26T18:00:00</sm:publicationDate>
    <owl:imports rdf:resource="http://www.omg.org/spec/EDMC-FIBO/FND/Agreements/Agreements/"/>
    <sm:dependsOn rdf:datatype="http://www.w3.org/2001/XMLSchema#anyURI"
    >http://www.omg.org/spec/EDMC-FIBO/FND/Agreements/Agreements/</sm:dependsOn>
    <dct:license rdf:resource="http://www.omg.org/spec/EDMC-FIBO/FND/Utilities/AnnotationVocabulary/MITLicense"/>
    <sm:topicArea rdf:datatype="http://www.w3.org/2001/XMLSchema#string"
    >finance</sm:topicArea>
    <sm:dependsOn rdf:datatype="http://www.w3.org/2001/XMLSchema#anyURI"
    >http://www.omg.org/spec/EDMC-FIBO/FND/Relations/Relations/</sm:dependsOn>
    <sm:specificationURL rdf:datatype="http://www.w3.org/2001/XMLSchema#anyURI"
    >http://www.omg.org/spec/EDMC-FIBO/FND/</sm:specificationURL>
  </owl:Ontology>
  <owl:Class rdf:about="http://www.omg.org/spec/EDMC-FIBO/FND/Agreements/Contracts/ContractualElement">
    <skos:editorialNote>The concept "contractual element" does not exist in any dictionary I could find. Can we change this to ContractElement? (efk)</skos:editorialNote>
    <skos:definition>Anything which relates to contracts.</skos:definition>
    <rdfs:label>contractual element</rdfs:label>
  </owl:Class>
  <owl:Class rdf:about="http://www.omg.org/spec/EDMC-FIBO/FND/Agreements/Contracts/ConditionsPrecedent">
    <rdfs:subClassOf>
      <owl:Class rdf:about="http://www.omg.org/spec/EDMC-FIBO/FND/Agreements/Contracts/ContractTermsSet"/>
    </rdfs:subClassOf>
    <skos:definition>Conditions precedent on some obligation. These are conditions which would alter the Obligation as it is otherwise stated.</skos:definition>
    <skos:editorialNote>Introduced for ISDA Master Agreement. It is likely that the Conditions Precedent defined for OTC Derivatives Master Agreements are actually applicable more widely. However, they are defined within the ISDA terms for now. Modeling note / review question: Modeled as a kind of Terms Set, combining terms and conditions. Should consider whether terms and conditions are distinct (Condition would then be a separate archetype).</skos:editorialNote>
    <rdfs:label>conditions precedent</rdfs:label>
  </owl:Class>
  <owl:Class rdf:about="http://www.omg.org/spec/EDMC-FIBO/FND/Agreements/Contracts/VerbalContract">
    <rdfs:subClassOf>
      <owl:Class rdf:about="http://www.omg.org/spec/EDMC-FIBO/FND/Agreements/Contracts/Contract"/>
    </rdfs:subClassOf>
    <skos:definition>A contract which exists as a result of some verbal exchange.</skos:definition>
    <rdfs:label>verbal contract</rdfs:label>
  </owl:Class>
  <owl:Class rdf:about="http://www.omg.org/spec/EDMC-FIBO/FND/Agreements/Contracts/Contract">
    <fibo-fnd-utl-av:definitionOrigin> http://www.businessdictionary.com/definition/contract.html</fibo-fnd-utl-av:definitionOrigin>
    <skos:definition>A voluntary, deliberate, and legally binding agreement between two or more competent parties. Contracts are usually written but may be spoken or implied, and generally have to do with employment, sale or lease, or tenancy.</skos:definition>
    <rdfs:subClassOf>
      <owl:Restriction>
        <owl:minQualifiedCardinality rdf:datatype="http://www.w3.org/2001/XMLSchema#nonNegativeInteger"
        >2</owl:minQualifiedCardinality>
        <owl:onClass rdf:resource="http://www.omg.org/spec/EDMC-FIBO/FND/Parties/Parties/PartyInRole"/>
        <owl:onProperty rdf:resource="http://www.omg.org/spec/EDMC-FIBO/FND/Parties/Parties/hasPartyInRole"/>
      </owl:Restriction>
    </rdfs:subClassOf>
    <rdfs:subClassOf>
      <owl:Restriction>
        <owl:qualifiedCardinality rdf:datatype="http://www.w3.org/2001/XMLSchema#nonNegativeInteger"
        >1</owl:qualifiedCardinality>
        <owl:onDataRange rdf:resource="http://www.omg.org/spec/EDMC-FIBO/FND/Utilities/BusinessFacingTypes/yesOrNo"/>
        <owl:onProperty>
          <owl:FunctionalProperty rdf:about="http://www.omg.org/spec/EDMC-FIBO/FND/Agreements/Contracts/isAssignable"/>
        </owl:onProperty>
      </owl:Restriction>
    </rdfs:subClassOf>
    <rdfs:subClassOf>
      <owl:Restriction>
        <owl:qualifiedCardinality rdf:datatype="http://www.w3.org/2001/XMLSchema#nonNegativeInteger"
        >1</owl:qualifiedCardinality>
        <owl:onDataRange rdf:resource="http://www.w3.org/2001/XMLSchema#dateTime"/>
        <owl:onProperty rdf:resource="http://www.omg.org/spec/EDMC-FIBO/FND/Relations/Relations/hasEffectiveDate"/>
      </owl:Restriction>
    </rdfs:subClassOf>
    <rdfs:label>contract</rdfs:label>
  </owl:Class>
  <owl:Class rdf:about="http://www.omg.org/spec/EDMC-FIBO/FND/Agreements/Contracts/BilateralContract">
    <skos:definition>A contract between two specific named parties. The rights and obligations pertaining to either party cannot be transferred to another party without prior written permission or a change to the contract itself.</skos:definition>
    <rdfs:subClassOf>
      <owl:Restriction>
        <owl:qualifiedCardinality rdf:datatype="http://www.w3.org/2001/XMLSchema#nonNegativeInteger"
        >2</owl:qualifiedCardinality>
        <owl:onClass rdf:resource="http://www.omg.org/spec/EDMC-FIBO/FND/Parties/Parties/PartyInRole"/>
        <owl:onProperty rdf:resource="http://www.omg.org/spec/EDMC-FIBO/FND/Parties/Parties/hasPartyInRole"/>
      </owl:Restriction>
    </rdfs:subClassOf>
    <rdfs:subClassOf rdf:resource="http://www.omg.org/spec/EDMC-FIBO/FND/Agreements/Contracts/Contract"/>
    <rdfs:label>bilateral contract</rdfs:label>
  </owl:Class>
  <owl:Class rdf:about="http://www.omg.org/spec/EDMC-FIBO/FND/Agreements/Contracts/PromissoryNote">
    <rdfs:subClassOf>
      <owl:Class rdf:about="http://www.omg.org/spec/EDMC-FIBO/FND/Agreements/Contracts/WrittenContract"/>
    </rdfs:subClassOf>
    <fibo-fnd-utl-av:definitionOrigin> http://www.businessdictionary.com/definition/promissory-note.html</fibo-fnd-utl-av:definitionOrigin>
    <skos:editorialNote>Unlike a contract, a Promissory Note does not need to be signed by both parties. It is essentiually a promise from one party to the holder, of some good or benefit. Promissory notes would generally by fully fungible. These are modeled as a kind of contract but are essentially a kind of unilateral contract between the issuer and the holder, and some authorities might not see this as a contract at all. Cash is a kind of promissory note, with the issuer being a central bank.</skos:editorialNote>
    <skos:definition>A promissory note is a written, signed, unconditional, and unsecured promise by one party (the maker or promisor) to another (the payee or promisee) that commits the maker to pay a specified sum on demand, or on a fixed or a determinable date. Promissory notes (such as bank or currency notes) are negotiable instruments.</skos:definition>
    <rdfs:label>promissory note</rdfs:label>
  </owl:Class>
  <owl:Class rdf:about="http://www.omg.org/spec/EDMC-FIBO/FND/Agreements/Contracts/NonBindingTermsSet">
    <skos:definition>Terms which do not have binding legal standing on the Issuer or Holder.</skos:definition>
    <rdfs:subClassOf>
      <owl:Class rdf:about="http://www.omg.org/spec/EDMC-FIBO/FND/Agreements/Contracts/ContractTermsSet"/>
    </rdfs:subClassOf>
    <rdfs:label>non-binding terms set</rdfs:label>
  </owl:Class>
  <owl:Class rdf:about="http://www.omg.org/spec/EDMC-FIBO/FND/Agreements/Contracts/ContractOriginator">
    <rdfs:subClassOf>
      <owl:Class rdf:about="http://www.omg.org/spec/EDMC-FIBO/FND/Agreements/Contracts/ContractPrincipal"/>
    </rdfs:subClassOf>
    <skos:definition>The party which originates the transferable contract and acts as the Principal in that contract regardless of the owner or counterparty.</skos:definition>
    <rdfs:label>contract originator</rdfs:label>
  </owl:Class>
  <owl:Class rdf:about="http://www.omg.org/spec/EDMC-FIBO/FND/Agreements/Contracts/WrittenContract">
    <owl:disjointWith rdf:resource="http://www.omg.org/spec/EDMC-FIBO/FND/Agreements/Contracts/VerbalContract"/>
    <rdfs:subClassOf rdf:resource="http://www.omg.org/spec/EDMC-FIBO/FND/Agreements/Contracts/Contract"/>
    <skos:definition>A formal Contract which is written and signed by both parties thereto.</skos:definition>
    <rdfs:label>written contract</rdfs:label>
  </owl:Class>
  <owl:Class rdf:about="http://www.omg.org/spec/EDMC-FIBO/FND/Agreements/Contracts/ContractualRelationship">
    <fibo-fnd-utl-av:definitionOrigin> http://www.businessdictionary.com/definition/contract.html</fibo-fnd-utl-av:definitionOrigin>
    <skos:definition>A contractual relationship is evidenced by (1) an offer, (2) acceptance of the offer, and a (3) valid (legal and valuable) consideration. Each party to a contract acquires rights and duties relative to the rights and duties of the other parties. However, while all parties may expect a fair benefit from the contract (otherwise courts may set it aside as inequitable) it does not follow that each party will benefit to an equal extent. Existence of contractual-relationship does not necessarily mean the contract is enforceable, or that it is not void (see void contract) or voidable (see voidable Contract).</skos:definition>
    <rdfs:label>contractual relationship</rdfs:label>
  </owl:Class>
  <owl:Class rdf:about="http://www.omg.org/spec/EDMC-FIBO/FND/Agreements/Contracts/ContractCounterparty">
    <skos:editorialNote>This term in Investopedia is named "counterparty" not "contract counterparty". Can we simplify this to "counterparty"? (efk)</skos:editorialNote>
    <fibo-fnd-utl-av:definitionOrigin> http://www.investopedia.com/terms/c/counterparty.asp</fibo-fnd-utl-av:definitionOrigin>
    <skos:definition>A counterparty is the other party that participates in a financial transaction.  Every transaction must have a counterparty in order for the transaction to go through. More specifically, every buyer of an asset must be paired up with a seller that is willing to sell and vice versa.</skos:definition>
    <rdfs:subClassOf rdf:resource="http://www.omg.org/spec/EDMC-FIBO/FND/Parties/Parties/PartyInRole"/>
    <rdfs:label>contract counterparty</rdfs:label>
  </owl:Class>
  <owl:Class rdf:about="http://www.omg.org/spec/EDMC-FIBO/FND/Agreements/Contracts/ContractTermsSet">
    <skos:editorialNote>The concept "contract terms set" does not exist in any dictionary I could find, however "terms and conditions" does, and could be used for this purpose. Can we change this to TermsAndConditions? If TermsAndConditions have parts, I would suggest creating a class called TermOrCondition, which would then provide the range for hasPart, and which could be specialized for various kinds of clauses, as appropriate.(efk)</skos:editorialNote>
    <fibo-fnd-utl-av:definitionOrigin> http://www.businessdictionary.com/definition/conditions-of-contract.html</fibo-fnd-utl-av:definitionOrigin>
    <fibo-fnd-utl-av:definitionOrigin> http://www.businessdictionary.com/definition/terms-and-conditions.html</fibo-fnd-utl-av:definitionOrigin>
    <skos:definition>The conditions of a contract include the terms and conditions that set the rights and obligations of the contracting parties when a contract is awarded or entered into.  These include general conditions which are common to all types of contracts, such as general and special arrangements, provisions, requirements, rules, specifications, and standards that form an integral part of an agreement or contract, as well as special conditions which are peculiar to a specific contract (such as, contract change conditions, payment conditions, price variation clauses, penalties).</skos:definition>
    <rdfs:subClassOf rdf:resource="http://www.omg.org/spec/EDMC-FIBO/FND/Agreements/Contracts/ContractualElement"/>
    <rdfs:subClassOf>
      <owl:Restriction>
        <owl:allValuesFrom rdf:resource="http://www.omg.org/spec/EDMC-FIBO/FND/Agreements/Contracts/ContractTermsSet"/>
        <owl:onProperty rdf:resource="http://www.omg.org/spec/EDMC-FIBO/FND/Relations/Relations/hasPart"/>
      </owl:Restriction>
    </rdfs:subClassOf>
    <rdfs:label>contract terms set</rdfs:label>
  </owl:Class>
  <owl:Class rdf:about="http://www.omg.org/spec/EDMC-FIBO/FND/Agreements/Contracts/TransferableContract">
    <fibo-fnd-utl-av:definitionOrigin>http://en.wikipedia.org/wiki/Assignment_(law)</fibo-fnd-utl-av:definitionOrigin>
    <skos:definition>An assignment (Latin cessio) is a term used with similar meanings in the law of contracts and in the law of real estate. In both instances, it encompasses the transfer of rights held by one party, the assignor, to another party, the assignee. The details of the assignment determines some additional rights and liabilities (or duties). Typically a third-party is involved in a contract with the assignor, and the contract is in effect transferred to the assignee.</skos:definition>
    <owl:equivalentClass>
      <owl:Restriction>
        <owl:minQualifiedCardinality rdf:datatype="http://www.w3.org/2001/XMLSchema#nonNegativeInteger"
        >1</owl:minQualifiedCardinality>
        <owl:onClass rdf:resource="http://www.omg.org/spec/EDMC-FIBO/FND/Agreements/Contracts/ContractOriginator"/>
        <owl:onProperty>
          <owl:ObjectProperty rdf:about="http://www.omg.org/spec/EDMC-FIBO/FND/Agreements/Contracts/hasPrincipal"/>
        </owl:onProperty>
      </owl:Restriction>
    </owl:equivalentClass>
    <rdfs:subClassOf>
      <owl:Restriction>
        <owl:minQualifiedCardinality rdf:datatype="http://www.w3.org/2001/XMLSchema#nonNegativeInteger"
        >1</owl:minQualifiedCardinality>
        <owl:onClass>
          <owl:Class rdf:about="http://www.omg.org/spec/EDMC-FIBO/FND/Agreements/Contracts/TransferableContractHolder"/>
        </owl:onClass>
        <owl:onProperty>
          <owl:ObjectProperty rdf:about="http://www.omg.org/spec/EDMC-FIBO/FND/Agreements/Contracts/hasCounterparty"/>
        </owl:onProperty>
      </owl:Restriction>
    </rdfs:subClassOf>
    <rdfs:subClassOf rdf:resource="http://www.omg.org/spec/EDMC-FIBO/FND/Agreements/Contracts/WrittenContract"/>
    <rdfs:label>transferable contract</rdfs:label>
  </owl:Class>
  <owl:Class rdf:about="http://www.omg.org/spec/EDMC-FIBO/FND/Agreements/Contracts/ContractualDefinition">
    <rdfs:subClassOf rdf:resource="http://www.omg.org/spec/EDMC-FIBO/FND/Agreements/Contracts/ContractualElement"/>
    <skos:editorialNote>The concept "contractual definition" does not exist in any dictionary I could find. Can we change this to ContractTermOrDefinition? (efk)</skos:editorialNote>
    <skos:editorialNote>These are agreed definitions which are then referred to in terms in contracts or other legal instruments.</skos:editorialNote>
    <skos:definition>The definition of something in some contract or other legal instrument.</skos:definition>
    <rdfs:label>contractual definition</rdfs:label>
  </owl:Class>
  <owl:Class rdf:about="http://www.omg.org/spec/EDMC-FIBO/FND/Agreements/Contracts/ContractPrincipal">
    <fibo-fnd-utl-av:definitionOrigin> http://www.businessdictionary.com/definition/principal.html</fibo-fnd-utl-av:definitionOrigin>
    <skos:definition>The party identified as being the principal or first party to a contract, in the event that the contract distinguishes any party as the principal. In law, the principal is the party that has the primary responsibility in a liability or obligation, as opposed to an endorser, guarantor, or surety.</skos:definition>
    <rdfs:subClassOf rdf:resource="http://www.omg.org/spec/EDMC-FIBO/FND/Parties/Parties/PartyInRole"/>
    <rdfs:label>contract principal</rdfs:label>
  </owl:Class>
  <owl:Class rdf:about="http://www.omg.org/spec/EDMC-FIBO/FND/Agreements/Contracts/ContractThirdParty">
    <skos:editorialNote>The concept "contract third party" does not exist in any dictionary I could find, however "third-party" does, and could be used for this purpose. Can we change this to ThirdParty? (efk)</skos:editorialNote>
    <fibo-fnd-utl-av:definitionOrigin> http://www.businessdictionary.com/definition/third-party.html</fibo-fnd-utl-av:definitionOrigin>
    <skos:definition>Someone who may be indirectly involved but is not a principal party to an arrangement, contract, deal, lawsuit, or transaction.</skos:definition>
    <rdfs:subClassOf rdf:resource="http://www.omg.org/spec/EDMC-FIBO/FND/Parties/Parties/PartyInRole"/>
    <rdfs:label>contract third party</rdfs:label>
  </owl:Class>
  <owl:Class rdf:about="http://www.omg.org/spec/EDMC-FIBO/FND/Agreements/Contracts/TransferableContractHolder">
    <rdfs:subClassOf rdf:resource="http://www.omg.org/spec/EDMC-FIBO/FND/Agreements/Contracts/ContractCounterparty"/>
    <skos:definition>The party which holds a transferable contract and enjoys the benefits defined in that contract while they hold it.</skos:definition>
    <skos:editorialNote>This party may transfer the contract to another party without reference to the issuer, for example by selling it in some marketplace.</skos:editorialNote>
    <rdfs:label>transferable contract holder</rdfs:label>
  </owl:Class>
  <owl:ObjectProperty rdf:about="http://www.omg.org/spec/EDMC-FIBO/FND/Agreements/Contracts/hasPrincipal">
    <rdfs:range rdf:resource="http://www.omg.org/spec/EDMC-FIBO/FND/Agreements/Contracts/ContractPrincipal"/>
    <rdfs:domain rdf:resource="http://www.omg.org/spec/EDMC-FIBO/FND/Agreements/Contracts/Contract"/>
    <rdfs:subPropertyOf rdf:resource="http://www.omg.org/spec/EDMC-FIBO/FND/Parties/Parties/hasPartyInRole"/>
    <skos:definition>identifies the main or principal party to a contract</skos:definition>
    <rdfs:label>has principal</rdfs:label>
  </owl:ObjectProperty>
  <owl:ObjectProperty rdf:about="http://www.omg.org/spec/EDMC-FIBO/FND/Agreements/Contracts/hasTerms">
    <rdfs:range rdf:resource="http://www.omg.org/spec/EDMC-FIBO/FND/Agreements/Contracts/ContractTermsSet"/>
    <rdfs:domain rdf:resource="http://www.omg.org/spec/EDMC-FIBO/FND/Agreements/Contracts/Contract"/>
    <rdfs:subPropertyOf rdf:resource="http://www.omg.org/spec/EDMC-FIBO/FND/Relations/Relations/has"/>
    <skos:definition>identifies a set of terms that form part of the contract. These are generally grouped for convenience as definitions, such as debt repayment terms, and may or may not equate to a formal clause, section, paragraph or other textual construct of the contract.</skos:definition>
    <rdfs:label>has terms</rdfs:label>
  </owl:ObjectProperty>
  <owl:ObjectProperty rdf:about="http://www.omg.org/spec/EDMC-FIBO/FND/Agreements/Contracts/supersedes">
    <rdfs:range rdf:resource="http://www.omg.org/spec/EDMC-FIBO/FND/Agreements/Contracts/Contract"/>
    <rdfs:domain rdf:resource="http://www.omg.org/spec/EDMC-FIBO/FND/Agreements/Contracts/WrittenContract"/>
    <skos:definition>The or any earlier contract which this written contract supersedes, whether that earlier contract is written or verbal or implied.</skos:definition>
    <rdfs:label>supersedes</rdfs:label>
  </owl:ObjectProperty>
  <owl:ObjectProperty rdf:about="http://www.omg.org/spec/EDMC-FIBO/FND/Agreements/Contracts/hasNonBindingTerms">
    <rdfs:range rdf:resource="http://www.omg.org/spec/EDMC-FIBO/FND/Agreements/Contracts/NonBindingTermsSet"/>
    <rdfs:domain rdf:resource="http://www.omg.org/spec/EDMC-FIBO/FND/Agreements/Contracts/Contract"/>
    <rdfs:subPropertyOf rdf:resource="http://www.omg.org/spec/EDMC-FIBO/FND/Agreements/Contracts/hasTerms"/>
    <skos:definition>refers to terms that are included in the contract but are not considered binding. In other words, a breach of such terms in the future would not be considered to be a breach of the contract.</skos:definition>
    <rdfs:label>has non-binding terms</rdfs:label>
  </owl:ObjectProperty>
  <owl:ObjectProperty rdf:about="http://www.omg.org/spec/EDMC-FIBO/FND/Agreements/Contracts/hasGoverningJurisdiction">
    <rdfs:range rdf:resource="http://www.omg.org/spec/EDMC-FIBO/FND/Law/Jurisdiction/Jurisdiction"/>
    <rdfs:domain rdf:resource="http://www.omg.org/spec/EDMC-FIBO/FND/Agreements/Contracts/Contract"/>
    <skos:editorialNote>As modeled, this relationship combines two slightly different senses in which a Jurisdiction may be named in some Contract: the jurisdiction under whose laws the contract is deemed to be in force, and the jurisdiction under which the parties agree to submit in the event of any dispute resolution. Scope Note: One thing to tease out is whether "Dispute Resolution" and other forms of "Governing Law" are one and the same thing or not. Dispute Resolution is uncontroversial, the question is whether there are other implications to Governing Law or if it's the same thing. For instance I may undertake to behave as though I were responsible to a particular authority i.e. a particular set of statutes.</skos:editorialNote>
    <skos:definition>identifies the jurisdiction governing the contract, as agreed by all parties. In a written contract this is generally identified, for example, as Governing Law, namely the jurisdiction in which any disputes arising from the contract are to be resolved.</skos:definition>
    <rdfs:subPropertyOf rdf:resource="http://www.omg.org/spec/EDMC-FIBO/FND/Relations/Relations/isGovernedBy"/>
    <rdfs:label>has governing jurisdiction</rdfs:label>
  </owl:ObjectProperty>
  <owl:ObjectProperty rdf:about="http://www.omg.org/spec/EDMC-FIBO/FND/Agreements/Contracts/hasThirdParty">
    <rdfs:range rdf:resource="http://www.omg.org/spec/EDMC-FIBO/FND/Agreements/Contracts/ContractThirdParty"/>
    <rdfs:domain rdf:resource="http://www.omg.org/spec/EDMC-FIBO/FND/Agreements/Contracts/Contract"/>
    <rdfs:subPropertyOf rdf:resource="http://www.omg.org/spec/EDMC-FIBO/FND/Parties/Parties/hasPartyInRole"/>
    <skos:definition>identifies a party which is not signatory to the party but has some role in the overall context defined by the contract.</skos:definition>
    <rdfs:label>has third party</rdfs:label>
  </owl:ObjectProperty>
  <owl:ObjectProperty rdf:about="http://www.omg.org/spec/EDMC-FIBO/FND/Agreements/Contracts/hasCounterparty">
    <rdfs:range rdf:resource="http://www.omg.org/spec/EDMC-FIBO/FND/Agreements/Contracts/ContractCounterparty"/>
    <rdfs:domain rdf:resource="http://www.omg.org/spec/EDMC-FIBO/FND/Agreements/Contracts/Contract"/>
    <rdfs:subPropertyOf rdf:resource="http://www.omg.org/spec/EDMC-FIBO/FND/Parties/Parties/hasPartyInRole"/>
    <skos:definition>identifies a counterparty to a contract</skos:definition>
    <rdfs:label>has counterparty</rdfs:label>
  </owl:ObjectProperty>
  <owl:ObjectProperty rdf:about="http://www.omg.org/spec/EDMC-FIBO/FND/Agreements/Contracts/definesTermsFor">
    <rdfs:domain rdf:resource="http://www.omg.org/spec/EDMC-FIBO/FND/Agreements/Contracts/Contract"/>
    <skos:changeNote>added to support requirements in Business Entities, 2013-05-22</skos:changeNote>
    <skos:definition>the contract sets out the terms for the something</skos:definition>
  </owl:ObjectProperty>
  <owl:FunctionalProperty rdf:about="http://www.omg.org/spec/EDMC-FIBO/FND/Agreements/Contracts/isAssignable">
    <skos:definition>indicates whether the contract and the rights thereunder may be assigned by one of the signatories to some other party</skos:definition>
    <rdfs:range rdf:resource="http://www.omg.org/spec/EDMC-FIBO/FND/Utilities/BusinessFacingTypes/yesOrNo"/>
    <rdf:type rdf:resource="http://www.w3.org/2002/07/owl#DatatypeProperty"/>
  </owl:FunctionalProperty>
</rdf:RDF>

<!-- Created with TopBraid -->
