<?xml version="1.0" encoding="UTF-8"?>
<!DOCTYPE rdf:RDF [
	<!ENTITY dct "http://purl.org/dc/terms/">
	<!ENTITY fibo-der-der-opt "https://spec.edmcouncil.org/fibo/ontology/DER/DerivativesContracts/Options/">
	<!ENTITY fibo-der-drc-bsc "https://spec.edmcouncil.org/fibo/ontology/DER/DerivativesContracts/DerivativesBasics/">
	<!ENTITY fibo-der-etd-eto "https://spec.edmcouncil.org/fibo/ontology/DER/ExchangeTradedDerivatives/ExchangeTradedOptions/">
	<!ENTITY fibo-der-sbd-eqo "https://spec.edmcouncil.org/fibo/ontology/DER/SecurityBasedDerivatives/EquityOptions/">
	<!ENTITY fibo-der-sbd-sbd "https://spec.edmcouncil.org/fibo/ontology/DER/SecurityBasedDerivatives/SecurityBasedDerivatives/">
	<!ENTITY fibo-fnd-acc-cur "https://spec.edmcouncil.org/fibo/ontology/FND/Accounting/CurrencyAmount/">
	<!ENTITY fibo-fnd-agr-ctr "https://spec.edmcouncil.org/fibo/ontology/FND/Agreements/Contracts/">
	<!ENTITY fibo-fnd-arr-arr "https://spec.edmcouncil.org/fibo/ontology/FND/Arrangements/Arrangements/">
	<!ENTITY fibo-fnd-law-jur "https://spec.edmcouncil.org/fibo/ontology/FND/Law/Jurisdiction/">
	<!ENTITY fibo-fnd-law-lcap "https://spec.edmcouncil.org/fibo/ontology/FND/Law/LegalCapacity/">
	<!ENTITY fibo-fnd-rel-rel "https://spec.edmcouncil.org/fibo/ontology/FND/Relations/Relations/">
	<!ENTITY fibo-fnd-utl-av "https://spec.edmcouncil.org/fibo/ontology/FND/Utilities/AnnotationVocabulary/">
	<!ENTITY fibo-ind-mkt-bas "https://spec.edmcouncil.org/fibo/ontology/IND/MarketIndices/BasketIndices/">
	<!ENTITY fibo-sec-eq-eq "https://spec.edmcouncil.org/fibo/ontology/SEC/Equities/EquityInstruments/">
	<!ENTITY owl "http://www.w3.org/2002/07/owl#">
	<!ENTITY rdf "http://www.w3.org/1999/02/22-rdf-syntax-ns#">
	<!ENTITY rdfs "http://www.w3.org/2000/01/rdf-schema#">
	<!ENTITY skos "http://www.w3.org/2004/02/skos/core#">
	<!ENTITY sm "http://www.omg.org/techprocess/ab/SpecificationMetadata/">
	<!ENTITY xsd "http://www.w3.org/2001/XMLSchema#">
]>
<rdf:RDF xml:base="https://spec.edmcouncil.org/fibo/ontology/DER/SecurityBasedDerivatives/EquityOptions/"
	xmlns:dct="http://purl.org/dc/terms/"
	xmlns:fibo-der-der-opt="https://spec.edmcouncil.org/fibo/ontology/DER/DerivativesContracts/Options/"
	xmlns:fibo-der-drc-bsc="https://spec.edmcouncil.org/fibo/ontology/DER/DerivativesContracts/DerivativesBasics/"
	xmlns:fibo-der-etd-eto="https://spec.edmcouncil.org/fibo/ontology/DER/ExchangeTradedDerivatives/ExchangeTradedOptions/"
	xmlns:fibo-der-sbd-eqo="https://spec.edmcouncil.org/fibo/ontology/DER/SecurityBasedDerivatives/EquityOptions/"
	xmlns:fibo-der-sbd-sbd="https://spec.edmcouncil.org/fibo/ontology/DER/SecurityBasedDerivatives/SecurityBasedDerivatives/"
	xmlns:fibo-fnd-acc-cur="https://spec.edmcouncil.org/fibo/ontology/FND/Accounting/CurrencyAmount/"
	xmlns:fibo-fnd-agr-ctr="https://spec.edmcouncil.org/fibo/ontology/FND/Agreements/Contracts/"
	xmlns:fibo-fnd-arr-arr="https://spec.edmcouncil.org/fibo/ontology/FND/Arrangements/Arrangements/"
	xmlns:fibo-fnd-law-jur="https://spec.edmcouncil.org/fibo/ontology/FND/Law/Jurisdiction/"
	xmlns:fibo-fnd-law-lcap="https://spec.edmcouncil.org/fibo/ontology/FND/Law/LegalCapacity/"
	xmlns:fibo-fnd-rel-rel="https://spec.edmcouncil.org/fibo/ontology/FND/Relations/Relations/"
	xmlns:fibo-fnd-utl-av="https://spec.edmcouncil.org/fibo/ontology/FND/Utilities/AnnotationVocabulary/"
	xmlns:fibo-ind-mkt-bas="https://spec.edmcouncil.org/fibo/ontology/IND/MarketIndices/BasketIndices/"
	xmlns:fibo-sec-eq-eq="https://spec.edmcouncil.org/fibo/ontology/SEC/Equities/EquityInstruments/"
	xmlns:owl="http://www.w3.org/2002/07/owl#"
	xmlns:rdf="http://www.w3.org/1999/02/22-rdf-syntax-ns#"
	xmlns:rdfs="http://www.w3.org/2000/01/rdf-schema#"
	xmlns:skos="http://www.w3.org/2004/02/skos/core#"
	xmlns:sm="http://www.omg.org/techprocess/ab/SpecificationMetadata/"
	xmlns:xsd="http://www.w3.org/2001/XMLSchema#">
	
	<owl:Ontology rdf:about="https://spec.edmcouncil.org/fibo/ontology/DER/SecurityBasedDerivatives/EquityOptions/">
		<rdfs:label xml:lang="en">Equity Options Ontology</rdfs:label>
		<dct:abstract>Options based on underlying equity instruments, baskets or indices. Additional terms specific to OTC equity options.</dct:abstract>
		<sm:fileAbbreviation>fibo-der-sbd-eqo</sm:fileAbbreviation>
		<owl:imports rdf:resource="https://spec.edmcouncil.org/fibo/ontology/DER/DerivativesContracts/DerivativesBasics/"/>
		<owl:imports rdf:resource="https://spec.edmcouncil.org/fibo/ontology/DER/DerivativesContracts/Options/"/>
		<owl:imports rdf:resource="https://spec.edmcouncil.org/fibo/ontology/DER/ExchangeTradedDerivatives/ExchangeTradedOptions/"/>
		<owl:imports rdf:resource="https://spec.edmcouncil.org/fibo/ontology/DER/SecurityBasedDerivatives/SecurityBasedDerivatives/"/>
		<owl:imports rdf:resource="https://spec.edmcouncil.org/fibo/ontology/FND/Accounting/CurrencyAmount/"/>
		<owl:imports rdf:resource="https://spec.edmcouncil.org/fibo/ontology/FND/Agreements/Contracts/"/>
		<owl:imports rdf:resource="https://spec.edmcouncil.org/fibo/ontology/FND/Arrangements/Arrangements/"/>
		<owl:imports rdf:resource="https://spec.edmcouncil.org/fibo/ontology/FND/Law/Jurisdiction/"/>
		<owl:imports rdf:resource="https://spec.edmcouncil.org/fibo/ontology/FND/Law/LegalCapacity/"/>
		<owl:imports rdf:resource="https://spec.edmcouncil.org/fibo/ontology/FND/Relations/Relations/"/>
		<owl:imports rdf:resource="https://spec.edmcouncil.org/fibo/ontology/FND/TransactionsExt/REATransactions/"/>
		<owl:imports rdf:resource="https://spec.edmcouncil.org/fibo/ontology/FND/TransactionsExt/SecuritiesTransactions/"/>
		<owl:imports rdf:resource="https://spec.edmcouncil.org/fibo/ontology/FND/Utilities/AnnotationVocabulary/"/>
		<owl:imports rdf:resource="https://spec.edmcouncil.org/fibo/ontology/IND/MarketIndices/BasketIndices/"/>
		<owl:imports rdf:resource="https://spec.edmcouncil.org/fibo/ontology/SEC/Equities/EquityInstruments/"/>
		<owl:versionIRI rdf:resource="https://spec.edmcouncil.org/fibo/ontology/DER/SecurityBasedDerivatives/EquityOptions/"/>
		<fibo-fnd-utl-av:hasMaturityLevel rdf:resource="&fibo-fnd-utl-av;Provisional"/>
	</owl:Ontology>
	
	<owl:Class rdf:about="&fibo-der-sbd-eqo;BasketOptionStrikeTerms">
		<rdfs:subClassOf rdf:resource="&fibo-der-sbd-eqo;EquityOptionExerciseTermsSet"/>
		<rdfs:label xml:lang="en">basket option strike terms</rdfs:label>
		<skos:definition xml:lang="en">Formal terms for the exercise of an Equity Basket Option. Further Notes Review 10 Feb: Strike price for Basket depends what is in the basket Single names: can come up with a value for the basket as a whole. Basket of Indices - would be different. Each constituent is an index. Basket that mixes single name as well as indices.</skos:definition>
	</owl:Class>
	
	<owl:Class rdf:about="&fibo-der-sbd-eqo;EquityBasketOptionOTCContract">
		<rdfs:subClassOf rdf:resource="&fibo-der-sbd-eqo;EquityOptionOTCContract"/>
		<rdfs:subClassOf>
			<owl:Restriction>
				<owl:onProperty rdf:resource="&fibo-der-drc-bsc;hasUnderlier"/>
				<owl:someValuesFrom rdf:resource="&fibo-der-sbd-sbd;EquityObservable"/>
			</owl:Restriction>
		</rdfs:subClassOf>
		<rdfs:subClassOf>
			<owl:Restriction>
				<owl:onProperty rdf:resource="&fibo-der-sbd-eqo;hasAnnex"/>
				<owl:someValuesFrom>
					<owl:Restriction>
						<owl:onProperty rdf:resource="&fibo-fnd-arr-arr;hasConstituent"/>
						<owl:someValuesFrom>
							<owl:Restriction>
								<owl:onProperty rdf:resource="&fibo-fnd-arr-arr;isConstituentOf"/>
								<owl:someValuesFrom rdf:resource="&fibo-ind-mkt-bas;BasketOfEquities"/>
							</owl:Restriction>
						</owl:someValuesFrom>
					</owl:Restriction>
				</owl:someValuesFrom>
			</owl:Restriction>
		</rdfs:subClassOf>
		<rdfs:label xml:lang="en">equity basket option o t c contract</rdfs:label>
	</owl:Class>
	
	<owl:Class rdf:about="&fibo-der-sbd-eqo;EquityIndexOptionOTCContract">
		<rdfs:subClassOf rdf:resource="&fibo-der-sbd-eqo;EquityOptionOTCContract"/>
		<rdfs:subClassOf>
			<owl:Restriction>
				<owl:onProperty rdf:resource="&fibo-der-drc-bsc;hasUnderlier"/>
				<owl:someValuesFrom>
					<owl:Restriction>
						<owl:onProperty rdf:resource="&fibo-fnd-rel-rel;hasIdentity"/>
						<owl:someValuesFrom rdf:resource="&fibo-ind-mkt-bas;ReferenceIndex"/>
					</owl:Restriction>
				</owl:someValuesFrom>
			</owl:Restriction>
		</rdfs:subClassOf>
		<rdfs:label xml:lang="en">equity index option o t c contract</rdfs:label>
		<skos:definition xml:lang="en">An option in which the underlyer is an equity index.</skos:definition>
		<skos:editorialNote xml:lang="en">Created to capture terms specific to index options. Note however that in FpML, there are no additional and different terms for basket options, so it maybe assumed that terms such as contract multiplier, which are defined for index options, are also applicable to basket options (a basket being a locally defined collection of securities which is otherwise similar to a published index of shares). Outcome of above question: see notes from 03 Feb review. The Basket Option must have an Annex which details the basket constituents. Also we are to add Contract types here for Basket Option contract and Custom Index Option.</skos:editorialNote>
	</owl:Class>
	
	<owl:Class rdf:about="&fibo-der-sbd-eqo;EquityIndexOptionStrikeTermsSet">
		<rdfs:subClassOf rdf:resource="&fibo-der-sbd-eqo;EquityOptionExerciseTermsSet"/>
		<rdfs:subClassOf>
			<owl:Restriction>
				<owl:onProperty rdf:resource="&fibo-der-sbd-eqo;includesSpecification"/>
				<owl:someValuesFrom rdf:resource="&fibo-der-der-opt;PercentageStrikePriceSpecification"/>
			</owl:Restriction>
		</rdfs:subClassOf>
		<rdfs:label xml:lang="en">equity index option strike terms set</rdfs:label>
		<skos:definition xml:lang="en">The strike price in respect of an index option transaction, is the level of the relevant index specified or otherwise determined in the transaction; This can be expressed either as a percentage of notional amount or as an absolute value.</skos:definition>
		<skos:editorialNote xml:lang="en">Adapted out of FpML equityStike (see original definition below); it is not clear whether the final provision in that definition (that the price can be expressed either as a percentage of notional or an absolute value) is intended to refer to index strike as well as single share option strike. REVIEW FpML equityStrike (complex type): A type for defining the strike price for an equity option. The strike price is either: (i) in respect of an index option transaction, the level of the relevant index specified or otherwise determined in the transaction; or (ii) in respect of a share option transaction, the price per share specified or otherwise determined in the transaction. This can be expressed either as a percentage of notional amount or as an absolute value.</skos:editorialNote>
	</owl:Class>
	
	<owl:Class rdf:about="&fibo-der-sbd-eqo;EquityOTCBasketOptionTransaction">
		<rdfs:subClassOf rdf:resource="&fibo-der-sbd-eqo;EquityOTCOptionTransaction"/>
		<rdfs:label xml:lang="en">equity o t c basket option transaction</rdfs:label>
	</owl:Class>
	
	<owl:Class rdf:about="&fibo-der-sbd-eqo;EquityOTCOptionTransaction">
		<rdfs:subClassOf rdf:resource="&fibo-der-drc-bsc;OTCDerivativeTransaction"/>
		<rdfs:subClassOf rdf:resource="&fibo-der-der-opt;OptionalUnderlyingTransaction"/>
		<rdfs:label xml:lang="en">equity o t c option transaction</rdfs:label>
		<skos:definition xml:lang="en">A transaction which is defined in an equity options contract and which may or may not take place, at the discretion of the holder of the option. If it does take place, this will be a transaction for the purchase or sale of the equity underlying or some cash equivalent thereof, as defined in the option contract.</skos:definition>
	</owl:Class>
	
	<owl:Class rdf:about="&fibo-der-sbd-eqo;EquityOptionCallTransaction">
		<rdfs:subClassOf rdf:resource="&fibo-der-der-opt;OptionCallTransaction"/>
		<rdfs:subClassOf rdf:resource="&fibo-der-sbd-eqo;EquityOTCOptionTransaction"/>
		<rdfs:label xml:lang="en">equity option call transaction</rdfs:label>
		<skos:definition xml:lang="en">A transaction which is defined in an equity options contract and which may or may not take place, at the discretion of the holder of the option. If it does take place, this will be a transaction for the purchase of the equity underlying or some cash equivalent thereof, as defined in the option contract.</skos:definition>
	</owl:Class>
	
	<owl:Class rdf:about="&fibo-der-sbd-eqo;EquityOptionEntitlement">
		<rdfs:subClassOf rdf:resource="&fibo-fnd-law-lcap;ContractualRight"/>
		<rdfs:label xml:lang="en">equity option entitlement</rdfs:label>
		<skos:definition xml:lang="en">The entitlements to the holder, comprised in an option contract or transaction supplement. FpML: &apos;The number of shares per option comprised in the option transaction supplement.&apos; In FpML this is an either / or: Either a whole number representing the number of shares per option, or a multiplier to be applied to an index underlyer (and, presumably, a basket underlyer)</skos:definition>
	</owl:Class>
	
	<owl:Class rdf:about="&fibo-der-sbd-eqo;EquityOptionExerciseTermsSet">
		<rdfs:subClassOf rdf:resource="&fibo-der-der-opt;OptionExerciseTimeTermsSet"/>
		<rdfs:label xml:lang="en">equity option exercise terms set</rdfs:label>
		<skos:definition xml:lang="en">Contractual terms setting out the price or level at which the Equity option is to be struck.</skos:definition>
		<fibo-fnd-utl-av:explanatoryNote xml:lang="en">FpML equityStrike (complex type): A type for defining the strike price for an equity option. The strike price is either: (i) in respect of an index option transaction, the level of the relevant index specified or otherwise determined in the transaction; or (ii) in respect of a share option transaction, the price per share specified or otherwise determined in the transaction. This can be expressed either as a percentage of notional amount or as an absolute value.</fibo-fnd-utl-av:explanatoryNote>
	</owl:Class>
	
	<owl:Class rdf:about="&fibo-der-sbd-eqo;EquityOptionOTCContract">
		<rdfs:subClassOf rdf:resource="&fibo-der-der-opt;OTCOptionContract"/>
		<rdfs:subClassOf rdf:resource="&fibo-der-sbd-sbd;EquityDerivative"/>
		<rdfs:subClassOf>
			<owl:Restriction>
				<owl:onProperty rdf:resource="&fibo-der-sbd-eqo;maySpecify"/>
				<owl:onClass rdf:resource="&fibo-der-etd-eto;ExchangeTradedOptionContract"/>
				<owl:maxQualifiedCardinality rdf:datatype="&xsd;nonNegativeInteger">1</owl:maxQualifiedCardinality>
			</owl:Restriction>
		</rdfs:subClassOf>
		<rdfs:subClassOf>
			<owl:Restriction>
				<owl:onProperty rdf:resource="&fibo-der-sbd-eqo;hasLocalJurisdiction"/>
				<owl:onClass rdf:resource="&fibo-fnd-law-jur;Jurisdiction"/>
				<owl:maxQualifiedCardinality rdf:datatype="&xsd;nonNegativeInteger">1</owl:maxQualifiedCardinality>
			</owl:Restriction>
		</rdfs:subClassOf>
		<rdfs:subClassOf>
			<owl:Restriction>
				<owl:onProperty rdf:resource="&fibo-der-drc-bsc;hasUnderlier"/>
				<owl:someValuesFrom rdf:resource="&fibo-der-sbd-sbd;EquityObservable"/>
			</owl:Restriction>
		</rdfs:subClassOf>
		<rdfs:subClassOf>
			<owl:Restriction>
				<owl:onProperty rdf:resource="&fibo-der-der-opt;definesOptional"/>
				<owl:someValuesFrom rdf:resource="&fibo-der-sbd-eqo;EquityOTCOptionTransaction"/>
			</owl:Restriction>
		</rdfs:subClassOf>
		<rdfs:subClassOf>
			<owl:Restriction>
				<owl:onProperty rdf:resource="&fibo-der-sbd-eqo;hasRelevantJurisdiction"/>
				<owl:someValuesFrom rdf:resource="&fibo-fnd-law-jur;Jurisdiction"/>
			</owl:Restriction>
		</rdfs:subClassOf>
		<rdfs:label xml:lang="en">equity option o t c contract</rdfs:label>
		<skos:definition xml:lang="en">Definition needed</skos:definition>
		<skos:editorialNote xml:lang="en">FpMl definition (unusable): A component describing an Equity Option product.</skos:editorialNote>
	</owl:Class>
	
	<owl:Class rdf:about="&fibo-der-sbd-eqo;EquityOptionPutTransaction">
		<rdfs:subClassOf rdf:resource="&fibo-der-der-opt;OptionPutTransaction"/>
		<rdfs:subClassOf rdf:resource="&fibo-der-sbd-eqo;EquityOTCOptionTransaction"/>
		<rdfs:label xml:lang="en">equity option put transaction</rdfs:label>
		<skos:definition xml:lang="en">A transaction which is defined in an equity options contract and which may or may not take place, at the discretion of the holder of the option. If it does take place, this will be a transaction for the sale of the equity underlying or some cash equivalent thereof, as defined in the option contract.</skos:definition>
	</owl:Class>
	
	<owl:Class rdf:about="&fibo-der-sbd-eqo;IndexOrBasketOptionEntitlement">
		<rdfs:subClassOf rdf:resource="&fibo-der-sbd-eqo;EquityOptionEntitlement"/>
		<rdfs:label xml:lang="en">index or basket option entitlement</rdfs:label>
		<skos:definition xml:lang="en">The entitlements to the holder of a basket or index option, comprised in an option contract or transaction supplement.</skos:definition>
	</owl:Class>
	
	<owl:Class rdf:about="&fibo-der-sbd-eqo;ShareOptionEntitlement">
		<rdfs:subClassOf rdf:resource="&fibo-der-sbd-eqo;EquityOptionEntitlement"/>
		<rdfs:label xml:lang="en">share option entitlement</rdfs:label>
		<skos:definition xml:lang="en">The entitlements to the holder of a single share option, comprised in an option contract or transaction supplement.</skos:definition>
	</owl:Class>
	
	<owl:Class rdf:about="&fibo-der-sbd-eqo;ShareOptionOTCContract">
		<rdfs:subClassOf rdf:resource="&fibo-der-sbd-eqo;EquityOptionOTCContract"/>
		<rdfs:subClassOf>
			<owl:Restriction>
				<owl:onProperty rdf:resource="&fibo-der-drc-bsc;hasUnderlier"/>
				<owl:someValuesFrom>
					<owl:Restriction>
						<owl:onProperty rdf:resource="&fibo-fnd-rel-rel;hasIdentity"/>
						<owl:someValuesFrom rdf:resource="&fibo-sec-eq-eq;ListedShare"/>
					</owl:Restriction>
				</owl:someValuesFrom>
			</owl:Restriction>
		</rdfs:subClassOf>
		<rdfs:label xml:lang="en">share option o t c contract</rdfs:label>
		<skos:definition xml:lang="en">An option in which the underlyer is a single publicly issued and traded share.</skos:definition>
	</owl:Class>
	
	<owl:Class rdf:about="&fibo-der-sbd-eqo;ShareOptionStrikeTermsSet">
		<rdfs:subClassOf rdf:resource="&fibo-der-sbd-eqo;EquityOptionExerciseTermsSet"/>
		<rdfs:subClassOf>
			<owl:Restriction>
				<owl:onProperty rdf:resource="&fibo-der-sbd-eqo;includesSpecification.1"/>
				<owl:someValuesFrom rdf:resource="&fibo-der-der-opt;AbsolutePriceStrikeSpecification"/>
			</owl:Restriction>
		</rdfs:subClassOf>
		<rdfs:label xml:lang="en">share option strike terms set</rdfs:label>
		<skos:definition xml:lang="en">The strike price is the price per share specified or otherwise determined in the transaction. This can be expressed either as a percentage of notional amount or as an absolute value. FpML equityStrike (complex type): A type for defining the strike price for an equity option. The strike price is either: (i) in respect of an index option transaction, the level of the relevant index specified or otherwise determined in the transaction; or (ii) in respect of a share option transaction, the price per share specified or otherwise determined in the transaction. This can be expressed either as a percentage of notional amount or as an absolute value.</skos:definition>
	</owl:Class>
	
	<owl:DatatypeProperty rdf:about="&fibo-der-sbd-eqo;contractMultiplier">
		<rdfs:label xml:lang="en">contract multiplier</rdfs:label>
		<rdfs:domain rdf:resource="&fibo-der-sbd-eqo;EquityIndexOptionOTCContract"/>
		<rdfs:range rdf:resource="&xsd;decimal"/>
		<skos:definition xml:lang="en">The contract multiplier associated with the index option.</skos:definition>
	</owl:DatatypeProperty>
	
	<owl:DatatypeProperty rdf:about="&fibo-der-sbd-eqo;exchangeLookalike">
		<rdfs:label xml:lang="en">exchange lookalike</rdfs:label>
		<rdfs:domain rdf:resource="&fibo-der-sbd-eqo;EquityOptionOTCContract"/>
		<rdfs:range rdf:resource="&xsd;boolean"/>
		<skos:definition xml:lang="en">Whether the corresponding transaction is to be treated as an &apos;exchange look-alike&apos;. If Yes, then the relevant share adjustments will follow that for a corresponding designated contract listed on the related exchange</skos:definition>
	</owl:DatatypeProperty>
	
	<owl:DatatypeProperty rdf:about="&fibo-der-sbd-eqo;extraordinaryEventsTreatment">
		<rdfs:label xml:lang="en">extraordinary events treatment</rdfs:label>
		<rdfs:domain rdf:resource="&fibo-der-sbd-eqo;ShareOptionOTCContract"/>
		<skos:definition xml:lang="en">Events affecting the issuer of those shares that may require the terms of the transaction to be adjusted.</skos:definition>
	</owl:DatatypeProperty>
	
	<owl:ObjectProperty rdf:about="&fibo-der-sbd-eqo;hasAnnex">
		<rdfs:subPropertyOf rdf:resource="&fibo-fnd-agr-ctr;hasContractualElement"/>
		<rdfs:label xml:lang="en">has annex</rdfs:label>
		<rdfs:domain rdf:resource="&fibo-der-sbd-eqo;EquityBasketOptionOTCContract"/>
	</owl:ObjectProperty>
	
	<owl:ObjectProperty rdf:about="&fibo-der-sbd-eqo;hasLocalJurisdiction">
		<rdfs:subPropertyOf rdf:resource="&fibo-fnd-agr-ctr;hasGoverningJurisdiction"/>
		<rdfs:label xml:lang="en">has local jurisdiction</rdfs:label>
		<rdfs:domain rdf:resource="&fibo-der-sbd-eqo;EquityOptionOTCContract"/>
		<rdfs:range rdf:resource="&fibo-fnd-law-jur;Jurisdiction"/>
	</owl:ObjectProperty>
	
	<owl:ObjectProperty rdf:about="&fibo-der-sbd-eqo;hasRelevantJurisdiction">
		<rdfs:subPropertyOf rdf:resource="&fibo-fnd-agr-ctr;hasGoverningJurisdiction"/>
		<rdfs:label xml:lang="en">has relevant jurisdiction</rdfs:label>
		<rdfs:domain rdf:resource="&fibo-der-sbd-eqo;EquityOptionOTCContract"/>
		<rdfs:range rdf:resource="&fibo-fnd-law-jur;Jurisdiction"/>
	</owl:ObjectProperty>
	
	<owl:ObjectProperty rdf:about="&fibo-der-sbd-eqo;includesSpecification">
		<rdfs:subPropertyOf rdf:resource="&fibo-der-der-opt;includesSpecificationTerm"/>
		<rdfs:label xml:lang="en">includes specification</rdfs:label>
		<rdfs:domain rdf:resource="&fibo-der-sbd-eqo;EquityIndexOptionStrikeTermsSet"/>
		<rdfs:range rdf:resource="&fibo-der-der-opt;PercentageStrikePriceSpecification"/>
	</owl:ObjectProperty>
	
	<owl:ObjectProperty rdf:about="&fibo-der-sbd-eqo;includesSpecification.1">
		<rdfs:subPropertyOf rdf:resource="&fibo-der-der-opt;includesSpecificationTerm"/>
		<rdfs:label xml:lang="en">includes specification</rdfs:label>
		<rdfs:domain rdf:resource="&fibo-der-sbd-eqo;ShareOptionStrikeTermsSet"/>
		<rdfs:range rdf:resource="&fibo-der-der-opt;AbsolutePriceStrikeSpecification"/>
	</owl:ObjectProperty>
	
	<owl:ObjectProperty rdf:about="&fibo-der-sbd-eqo;maySpecify">
		<rdfs:label xml:lang="en">may specify</rdfs:label>
		<rdfs:domain rdf:resource="&fibo-der-sbd-eqo;EquityOptionOTCContract"/>
		<rdfs:range rdf:resource="&fibo-der-etd-eto;ExchangeTradedOptionContract"/>
	</owl:ObjectProperty>
	
	<owl:DatatypeProperty rdf:about="&fibo-der-sbd-eqo;multiplier">
		<rdfs:label xml:lang="en">multiplier</rdfs:label>
		<rdfs:domain rdf:resource="&fibo-der-sbd-eqo;IndexOrBasketOptionEntitlement"/>
		<rdfs:range rdf:resource="&xsd;decimal"/>
		<skos:definition xml:lang="en">The contract multiplier associated with an index or basket option.</skos:definition>
	</owl:DatatypeProperty>
	
	<owl:DatatypeProperty rdf:about="&fibo-der-sbd-eqo;nearestIndexProvision">
		<rdfs:label xml:lang="en">nearest index provision</rdfs:label>
		<rdfs:domain rdf:resource="&fibo-der-sbd-eqo;EquityBasketOptionOTCContract"/>
		<rdfs:range rdf:resource="&xsd;boolean"/>
		<skos:definition xml:lang="en">For an index option transaction, whether the Nearest Index Contract provision is applicable.</skos:definition>
	</owl:DatatypeProperty>
	
	<owl:ObjectProperty rdf:about="&fibo-der-sbd-eqo;notionalAmount">
		<rdfs:label xml:lang="en">notional amount</rdfs:label>
		<rdfs:domain rdf:resource="&fibo-der-sbd-eqo;EquityOptionOTCContract"/>
		<rdfs:range rdf:resource="&fibo-fnd-acc-cur;MonetaryAmount"/>
		<skos:definition xml:lang="en">&apos;The notional amount.&apos; Further notes: Presumably all options have a notional amount. This is defined here for Eqiuty Option. FpML: &apos;The notional amount.&apos;</skos:definition>
	</owl:ObjectProperty>
	
	<owl:DatatypeProperty rdf:about="&fibo-der-sbd-eqo;novationAllowable">
		<rdfs:label xml:lang="en">novation allowable</rdfs:label>
		<rdfs:domain rdf:resource="&fibo-der-sbd-eqo;EquityOptionOTCContract"/>
		<rdfs:range rdf:resource="&xsd;boolean"/>
	</owl:DatatypeProperty>
	
	<owl:DatatypeProperty rdf:about="&fibo-der-sbd-eqo;novationRequired">
		<rdfs:label xml:lang="en">novation required</rdfs:label>
		<rdfs:domain rdf:resource="&fibo-der-sbd-eqo;EquityOptionOTCContract"/>
		<rdfs:range rdf:resource="&xsd;boolean"/>
	</owl:DatatypeProperty>
	
	<owl:DatatypeProperty rdf:about="&fibo-der-sbd-eqo;numberOfOptions">
		<rdfs:label xml:lang="en">number of options</rdfs:label>
		<rdfs:domain rdf:resource="&fibo-der-sbd-eqo;EquityOptionOTCContract"/>
		<rdfs:range rdf:resource="&xsd;decimal"/>
		<skos:definition xml:lang="en">The price per equity security, index or basket observed on the trade or effective date. FpML: &apos;The price per asset, index or basket observed on the trade or effective date.&apos;</skos:definition>
	</owl:DatatypeProperty>
	
	<owl:DatatypeProperty rdf:about="&fibo-der-sbd-eqo;numberOfShares">
		<rdfs:label xml:lang="en">number of shares</rdfs:label>
		<rdfs:domain rdf:resource="&fibo-der-sbd-eqo;ShareOptionEntitlement"/>
		<rdfs:range rdf:resource="&xsd;decimal"/>
		<skos:definition xml:lang="en">The number of shares per option comprised in the option. FpML: &apos;The number of shares per option comprised in the option transaction supplement.&apos;</skos:definition>
	</owl:DatatypeProperty>
	
	<owl:DatatypeProperty rdf:about="&fibo-der-sbd-eqo;sharesPerOption">
		<rdfs:label xml:lang="en">shares per option</rdfs:label>
		<rdfs:domain rdf:resource="&fibo-der-sbd-eqo;ShareOptionOTCContract"/>
		<rdfs:range rdf:resource="&xsd;integer"/>
		<skos:definition xml:lang="en">The number of shares per option defined for the option contract.</skos:definition>
	</owl:DatatypeProperty>

</rdf:RDF>