<?xml version="1.0" encoding="UTF-8"?>
<!DOCTYPE rdf:RDF [
	<!ENTITY dct "http://purl.org/dc/terms/">
	<!ENTITY fibo-der-der-rsw "https://spec.edmcouncil.org/fibo/ontology/DER/DerivativesContracts/ReturnSwaps/">
	<!ENTITY fibo-der-drc-bsc "https://spec.edmcouncil.org/fibo/ontology/DER/DerivativesContracts/DerivativesBasics/">
	<!ENTITY fibo-der-drc-swp "https://spec.edmcouncil.org/fibo/ontology/DER/DerivativesContracts/Swaps/">
	<!ENTITY fibo-der-sbd-eqs "https://spec.edmcouncil.org/fibo/ontology/DER/SecurityBasedDerivatives/EquitySwaps/">
	<!ENTITY fibo-der-sbd-sbd "https://spec.edmcouncil.org/fibo/ontology/DER/SecurityBasedDerivatives/SecurityBasedDerivatives/">
	<!ENTITY fibo-fnd-acc-cur "https://spec.edmcouncil.org/fibo/ontology/FND/Accounting/CurrencyAmount/">
	<!ENTITY fibo-fnd-rel-rel "https://spec.edmcouncil.org/fibo/ontology/FND/Relations/Relations/">
	<!ENTITY fibo-fnd-utl-alx "https://spec.edmcouncil.org/fibo/ontology/FND/Utilities/Analytics/">
	<!ENTITY fibo-fnd-utl-av "https://spec.edmcouncil.org/fibo/ontology/FND/Utilities/AnnotationVocabulary/">
	<!ENTITY fibo-ind-mkt-bas "https://spec.edmcouncil.org/fibo/ontology/IND/MarketIndices/BasketIndices/">
	<!ENTITY fibo-sec-eq-eq "https://spec.edmcouncil.org/fibo/ontology/SEC/Equities/EquityInstruments/">
	<!ENTITY owl "http://www.w3.org/2002/07/owl#">
	<!ENTITY rdf "http://www.w3.org/1999/02/22-rdf-syntax-ns#">
	<!ENTITY rdfs "http://www.w3.org/2000/01/rdf-schema#">
	<!ENTITY skos "http://www.w3.org/2004/02/skos/core#">
	<!ENTITY sm "http://www.omg.org/techprocess/ab/SpecificationMetadata/">
	<!ENTITY xsd "http://www.w3.org/2001/XMLSchema#">
]>
<rdf:RDF xml:base="https://spec.edmcouncil.org/fibo/ontology/DER/SecurityBasedDerivatives/EquitySwaps/"
	xmlns:dct="http://purl.org/dc/terms/"
	xmlns:fibo-der-der-rsw="https://spec.edmcouncil.org/fibo/ontology/DER/DerivativesContracts/ReturnSwaps/"
	xmlns:fibo-der-drc-bsc="https://spec.edmcouncil.org/fibo/ontology/DER/DerivativesContracts/DerivativesBasics/"
	xmlns:fibo-der-drc-swp="https://spec.edmcouncil.org/fibo/ontology/DER/DerivativesContracts/Swaps/"
	xmlns:fibo-der-sbd-eqs="https://spec.edmcouncil.org/fibo/ontology/DER/SecurityBasedDerivatives/EquitySwaps/"
	xmlns:fibo-der-sbd-sbd="https://spec.edmcouncil.org/fibo/ontology/DER/SecurityBasedDerivatives/SecurityBasedDerivatives/"
	xmlns:fibo-fnd-acc-cur="https://spec.edmcouncil.org/fibo/ontology/FND/Accounting/CurrencyAmount/"
	xmlns:fibo-fnd-rel-rel="https://spec.edmcouncil.org/fibo/ontology/FND/Relations/Relations/"
	xmlns:fibo-fnd-utl-alx="https://spec.edmcouncil.org/fibo/ontology/FND/Utilities/Analytics/"
	xmlns:fibo-fnd-utl-av="https://spec.edmcouncil.org/fibo/ontology/FND/Utilities/AnnotationVocabulary/"
	xmlns:fibo-ind-mkt-bas="https://spec.edmcouncil.org/fibo/ontology/IND/MarketIndices/BasketIndices/"
	xmlns:fibo-sec-eq-eq="https://spec.edmcouncil.org/fibo/ontology/SEC/Equities/EquityInstruments/"
	xmlns:owl="http://www.w3.org/2002/07/owl#"
	xmlns:rdf="http://www.w3.org/1999/02/22-rdf-syntax-ns#"
	xmlns:rdfs="http://www.w3.org/2000/01/rdf-schema#"
	xmlns:skos="http://www.w3.org/2004/02/skos/core#"
	xmlns:sm="http://www.omg.org/techprocess/ab/SpecificationMetadata/"
	xmlns:xsd="http://www.w3.org/2001/XMLSchema#">
	
	<owl:Ontology rdf:about="https://spec.edmcouncil.org/fibo/ontology/DER/SecurityBasedDerivatives/EquitySwaps/">
		<rdfs:label xml:lang="en">EquitySwaps</rdfs:label>
		<dct:abstract>Swap contracts in which one leg gives some form of return on an equity asset, including dividend returns, total asset returns equity dispersion and correlation measurement terms. Many of these return calculations are based on a variety of calculation methods and may vary widely.</dct:abstract>
		<sm:fileAbbreviation>fibo-der-sbd-eqs</sm:fileAbbreviation>
		<owl:imports rdf:resource="https://spec.edmcouncil.org/fibo/ontology/DER/DerivativesContracts/DerivativesBasics/"/>
		<owl:imports rdf:resource="https://spec.edmcouncil.org/fibo/ontology/DER/DerivativesContracts/ReturnSwaps/"/>
		<owl:imports rdf:resource="https://spec.edmcouncil.org/fibo/ontology/DER/DerivativesContracts/Swaps/"/>
		<owl:imports rdf:resource="https://spec.edmcouncil.org/fibo/ontology/DER/SecurityBasedDerivatives/SecurityBasedDerivatives/"/>
		<owl:imports rdf:resource="https://spec.edmcouncil.org/fibo/ontology/FBC/FinancialInstruments/FinancialInstruments/"/>
		<owl:imports rdf:resource="https://spec.edmcouncil.org/fibo/ontology/FND/Accounting/CurrencyAmount/"/>
		<owl:imports rdf:resource="https://spec.edmcouncil.org/fibo/ontology/FND/Relations/Relations/"/>
		<owl:imports rdf:resource="https://spec.edmcouncil.org/fibo/ontology/FND/TransactionsExt/REATransactions/"/>
		<owl:imports rdf:resource="https://spec.edmcouncil.org/fibo/ontology/FND/Utilities/Analytics/"/>
		<owl:imports rdf:resource="https://spec.edmcouncil.org/fibo/ontology/FND/Utilities/AnnotationVocabulary/"/>
		<owl:imports rdf:resource="https://spec.edmcouncil.org/fibo/ontology/IND/MarketIndices/BasketIndices/"/>
		<owl:imports rdf:resource="https://spec.edmcouncil.org/fibo/ontology/SEC/Equities/EquityInstruments/"/>
		<owl:versionIRI rdf:resource="https://spec.edmcouncil.org/fibo/ontology/DER/SecurityBasedDerivatives/EquitySwaps/"/>
		<fibo-fnd-utl-av:hasMaturityLevel rdf:resource="&fibo-fnd-utl-av;Provisional"/>
	</owl:Ontology>
	
	<owl:Class rdf:about="&fibo-der-sbd-eqs;CorrelationLegTerms">
		<rdfs:subClassOf rdf:resource="&fibo-der-sbd-sbd;PerformanceBasedVariableLeg"/>
		<rdfs:subClassOf>
			<owl:Restriction>
				<owl:onProperty rdf:resource="&fibo-der-drc-bsc;hasUnderlier"/>
				<owl:someValuesFrom>
					<owl:Restriction>
						<owl:onProperty rdf:resource="&fibo-fnd-rel-rel;hasIdentity"/>
						<owl:someValuesFrom rdf:resource="&fibo-ind-mkt-bas;ReferenceIndex"/>
					</owl:Restriction>
				</owl:someValuesFrom>
			</owl:Restriction>
		</rdfs:subClassOf>
		<rdfs:subClassOf>
			<owl:Restriction>
				<owl:onProperty rdf:resource="&fibo-fnd-acc-cur;hasNotionalAmount"/>
				<owl:someValuesFrom rdf:resource="&fibo-fnd-acc-cur;MonetaryAmount"/>
			</owl:Restriction>
		</rdfs:subClassOf>
		<rdfs:label xml:lang="en">correlation leg terms</rdfs:label>
		<skos:definition xml:lang="en">Definition needed. FpML refers to this but does not define its meaning. Correslation between two prices</skos:definition>
		<fibo-fnd-utl-av:explanatoryNote xml:lang="en">Correlation Buyer is deemed to be the Equity Amount Receiver, Correlation Seller is deemed to be the Equity Amount Payer. FpML: &apos;Correlation Leg. Correlation Buyer is deemed to be the Equity Amount Receiver, Correlation Seller is deemed to be the Equity Amount Payer.&apos;</fibo-fnd-utl-av:explanatoryNote>
	</owl:Class>
	
	<owl:Class rdf:about="&fibo-der-sbd-eqs;CovarianceLegTerms">
		<rdfs:subClassOf rdf:resource="&fibo-der-sbd-sbd;PerformanceBasedVariableLeg"/>
		<rdfs:label xml:lang="en">covariance leg terms</rdfs:label>
		<skos:definition xml:lang="en">A statistical leg based on covariance. REVIEW: This kmight specify the same kind of thing as Correlation Leg using different mathematics / different legal terms (in which case we need to model it as a different thing even though to the investor it has the same rationale and behavior. The relative movement of one thing to the other over a period of time. So this adds a time base to the Correlation calculation. difference with Correelation: The time base in correlation swap is implicit anyway (it&apos;s the duration of the contract. so Covariance is what allows you to explan x% of the vaqriabiltiy of the price of this asset with relation to that asset.</skos:definition>
		<skos:editorialNote xml:lang="en">Original review note: Co-variance Leg Another statistical swap leg type where the stike determines the payout. Structured the same as the Correlation Leg. more notes 17 March: Covariane is actually the way you measure correlation. So people talk about this as a statistical leg but actually Talks about movement of price THe highter the covariance between two prices the more correlated they are. more general note: unlike fx market where e.g. I cna build a price out od AUS/USD and build a price out of that. In option markets I don&apos;t have that opportunity - one owiuld end up overpricing the option. The variability in the price of AUS/USD v AUS/GBP impacts on these calculations. By using three legs I cna put together a cros inthe options. Buy Aus/USD Option, .buy USD/GBP Option and sell the correlation Swap. This sells the correlationbeteen AUS/USD and AUS/GBP leaving me with a realistic price for AUS/GBP thereby enabling me to cross markets. So the swap enables me not to end up overpricing the option. THis basic principle is why correslation swaps are used. So correslation is a relatively new concept.</skos:editorialNote>
	</owl:Class>
	
	<owl:Class rdf:about="&fibo-der-sbd-eqs;DispersionLeg">
		<rdfs:subClassOf rdf:resource="&fibo-der-sbd-sbd;PerformanceBasedVariableLeg"/>
		<rdfs:label xml:lang="en">dispersion leg</rdfs:label>
		<skos:definition xml:lang="en">leg of a dispersion swap</skos:definition>
		<fibo-fnd-utl-av:explanatoryNote xml:lang="en">Both legs are Return Legs, there is no Payment Leg. Model review notes: Dispersion Swap is a basket, where the constituents of the basket would typically include indices. So it may be Long the index and short the top 20 constituents of that index. Typically index v some form of the constituents, is what makes up a dispersion swap. Also (statistical swaps) - Market Disruption Event. For instance - define what dates are observed, so some dates get dropped due to market disruption events There would be some contractual terms about this, defining for instance the kinds of events defined as market disruptions, and the fact that the dates when these happen, these observations are not made. Look at examples.</fibo-fnd-utl-av:explanatoryNote>
	</owl:Class>
	
	<owl:Class rdf:about="&fibo-der-sbd-eqs;DispersionSwapContract">
		<rdfs:subClassOf rdf:resource="&fibo-der-drc-swp;Swap"/>
		<rdfs:label xml:lang="en">dispersion swap contract</rdfs:label>
	</owl:Class>
	
	<owl:Class rdf:about="&fibo-der-sbd-eqs;DispersionSwapIndexConstituentsLegTerms">
		<rdfs:subClassOf rdf:resource="&fibo-der-sbd-eqs;DispersionLeg"/>
		<rdfs:subClassOf>
			<owl:Restriction>
				<owl:onProperty rdf:resource="&fibo-der-drc-bsc;hasUnderlier"/>
				<owl:someValuesFrom>
					<owl:Restriction>
						<owl:onProperty rdf:resource="&fibo-fnd-rel-rel;hasIdentity"/>
						<owl:someValuesFrom rdf:resource="&fibo-ind-mkt-bas;BasketOfEquities"/>
					</owl:Restriction>
				</owl:someValuesFrom>
			</owl:Restriction>
		</rdfs:subClassOf>
		<rdfs:label xml:lang="en">dispersion swap index constituents leg terms</rdfs:label>
		<skos:definition xml:lang="en">The side of a dispersion swap where the underlying is a defined sub-set of an index, i.e. a set of constituents of that index.</skos:definition>
	</owl:Class>
	
	<owl:Class rdf:about="&fibo-der-sbd-eqs;DispersionSwapIndexLegTerms">
		<rdfs:subClassOf rdf:resource="&fibo-der-sbd-eqs;DispersionLeg"/>
		<rdfs:subClassOf>
			<owl:Restriction>
				<owl:onProperty rdf:resource="&fibo-der-drc-bsc;hasUnderlier"/>
				<owl:someValuesFrom>
					<owl:Restriction>
						<owl:onProperty rdf:resource="&fibo-fnd-rel-rel;hasIdentity"/>
						<owl:someValuesFrom rdf:resource="&fibo-ind-mkt-bas;ReferenceIndex"/>
					</owl:Restriction>
				</owl:someValuesFrom>
			</owl:Restriction>
		</rdfs:subClassOf>
		<rdfs:label xml:lang="en">dispersion swap index leg terms</rdfs:label>
		<skos:definition xml:lang="en">The side of a dispersion swap which has a particular index as its underlying. Further notes: This is a leg of a dispersion swap, which is defined by the index itself. This may be set against the other leg which is made up of a defined part of that index. Review comment: aren&apos;t really legs.</skos:definition>
	</owl:Class>
	
	<owl:Class rdf:about="&fibo-der-sbd-eqs;DispersionSwapTransaction">
		<rdfs:subClassOf>
			<owl:Restriction>
				<owl:onProperty rdf:resource="&fibo-der-drc-swp;hasLeg"/>
				<owl:onClass rdf:resource="&fibo-der-sbd-eqs;DispersionLeg"/>
				<owl:qualifiedCardinality rdf:datatype="&xsd;nonNegativeInteger">2</owl:qualifiedCardinality>
			</owl:Restriction>
		</rdfs:subClassOf>
		<rdfs:label xml:lang="en">dispersion swap transaction</rdfs:label>
	</owl:Class>
	
	<owl:Class rdf:about="&fibo-der-sbd-eqs;DividendConditions">
		<rdfs:label xml:lang="en">dividend conditions</rdfs:label>
		<skos:definition xml:lang="en">Conditions governing the payment of dividends to the receiver of the equity forward.</skos:definition>
		<skos:editorialNote xml:lang="en">FpML has a set of terms for Dividend Conditions which are usable across a range of derivatives, including Forward. Many of the definitions of individual terms refer specifically to equity return (swaps) and it is not clear whether each such term also applies to Equity forwards (i.e. the definition is more specific than it should be), or if these are terms unique to Equity Return Swaps, among which are terms applicable to Equity forwards. REVIEW: 19 May: If you have a forward contract with a dividend before you settle there must be some terms to determine how the dividend is resolved. Similar question would apply with Bond Interst? No becaues this is a known amount so it is taken into account in the price that&apos;s been agreed (discount premium). Whether it&apos;s cum or ex coupon therefore doesn&apos;t affect pricing; with Dividend this is not the case, there afore there are contractual trerms about how that is to be resolved. FpML: A type describing the conditions governing the payment of dividends to the receiver of the equity return. With the exception of the dividend payout ratio, which is defined for each of the underlying components.</skos:editorialNote>
	</owl:Class>
	
	<owl:Class rdf:about="&fibo-der-sbd-eqs;DividendLegDividendPeriod">
		<rdfs:subClassOf>
			<owl:Restriction>
				<owl:onProperty rdf:resource="&fibo-der-sbd-eqs;hasSomeDividendPeriods"/>
				<owl:someValuesFrom rdf:resource="&fibo-der-sbd-eqs;DividendPeriod"/>
			</owl:Restriction>
		</rdfs:subClassOf>
		<rdfs:label xml:lang="en">dividend leg dividend period</rdfs:label>
		<skos:definition xml:lang="en">A part of a Dividend Leg, which is the dividend period and the terms relating to this.</skos:definition>
	</owl:Class>
	
	<owl:Class rdf:about="&fibo-der-sbd-eqs;DividendPeriod">
		<rdfs:label xml:lang="en">dividend period</rdfs:label>
		<skos:definition xml:lang="en">A dividend payment period.</skos:definition>
	</owl:Class>
	
	<owl:Class rdf:about="&fibo-der-sbd-eqs;DividendStream">
		<rdfs:subClassOf rdf:resource="&fibo-der-der-rsw;SimpleReturnStream"/>
		<rdfs:subClassOf>
			<owl:Restriction>
				<owl:onProperty rdf:resource="&fibo-der-sbd-eqs;hasComponent.1"/>
				<owl:onClass rdf:resource="&fibo-der-sbd-eqs;SpecialDividendLegTerm"/>
				<owl:maxQualifiedCardinality rdf:datatype="&xsd;nonNegativeInteger">1</owl:maxQualifiedCardinality>
			</owl:Restriction>
		</rdfs:subClassOf>
		<rdfs:subClassOf>
			<owl:Restriction>
				<owl:onProperty rdf:resource="&fibo-der-drc-bsc;hasUnderlier"/>
				<owl:someValuesFrom>
					<owl:Restriction>
						<owl:onProperty rdf:resource="&fibo-fnd-rel-rel;hasIdentity"/>
						<owl:someValuesFrom rdf:resource="&fibo-sec-eq-eq;ListedShare"/>
					</owl:Restriction>
				</owl:someValuesFrom>
			</owl:Restriction>
		</rdfs:subClassOf>
		<rdfs:subClassOf>
			<owl:Restriction>
				<owl:onProperty rdf:resource="&fibo-der-der-rsw;hasReferenceAsset"/>
				<owl:someValuesFrom rdf:resource="&fibo-der-sbd-sbd;EquityObservable"/>
			</owl:Restriction>
		</rdfs:subClassOf>
		<rdfs:subClassOf>
			<owl:Restriction>
				<owl:onProperty rdf:resource="&fibo-der-sbd-eqs;hasComponent"/>
				<owl:someValuesFrom rdf:resource="&fibo-der-sbd-eqs;DividendLegDividendPeriod"/>
			</owl:Restriction>
		</rdfs:subClassOf>
		<rdfs:label xml:lang="en">dividend stream</rdfs:label>
		<skos:definition xml:lang="en">The Floating Payment Leg of a Dividend Swap. Swap dividend payment rates. Earlier notes this behaves very like a variance swap but instead of betting in pure variance you take a bet on dividend. What practically in one of these: The difference between th ereal life dividend and the one you think it should be. so I say it should bte 2% over the next 10 years, so I swap 2% for the actual dividend amount So then there is one single payment at the end which nets these up. So in the above example ... they are usually 3 month or 6 month contracts, so if for instance th edividend if quarterly, there might be 2 dividends where the difference is netted up at the end.for example. (Us 1/4ly usually , Eur 6 months). Depends on the company&apos;s articles of association etc. e.g. Unilever is 6 mo)/ Structurally, Div Swap corr Swap and Var Swap are structured similarly, with one strike at the beginning. Strike may be expressed in terms of the (price) variance (the variance of the returns) , the correlation between typically 2 underlyers. or the dividend for each of these three types of swap respectively. 17 march Dividend is a flow based on a share, so is this not the same as a Return Swap in that the dividend is the return on the dividend? Also recall that with stocks themselves, there is no comitment by the issuer to pay the dividends. FpML: &apos;Dividend leg.&apos;; &apos;Floating Payment Leg of a Dividend Swap.&apos;</skos:definition>
	</owl:Class>
	
	<owl:Class rdf:about="&fibo-der-sbd-eqs;EquityCorrelationSwapContract">
		<rdfs:subClassOf rdf:resource="&fibo-der-sbd-sbd;EquityDerivative"/>
		<rdfs:subClassOf rdf:resource="&fibo-der-sbd-sbd;StatisticalSwap"/>
		<rdfs:subClassOf>
			<owl:Restriction>
				<owl:onProperty rdf:resource="&fibo-der-drc-bsc;hasUnderlier"/>
				<owl:someValuesFrom>
					<owl:Restriction>
						<owl:onProperty rdf:resource="&fibo-fnd-rel-rel;hasIdentity"/>
						<owl:someValuesFrom rdf:resource="&fibo-ind-mkt-bas;ReferenceIndex"/>
					</owl:Restriction>
				</owl:someValuesFrom>
			</owl:Restriction>
		</rdfs:subClassOf>
		<rdfs:label xml:lang="en">equity correlation swap contract</rdfs:label>
		<skos:definition xml:lang="en">no definition FpML (unusable): A correlation swap.</skos:definition>
	</owl:Class>
	
	<owl:Class rdf:about="&fibo-der-sbd-eqs;EquityDividendSwap">
		<rdfs:subClassOf rdf:resource="&fibo-der-drc-swp;Swap"/>
		<rdfs:subClassOf rdf:resource="&fibo-der-sbd-sbd;EquityDerivative"/>
		<rdfs:subClassOf>
			<owl:Restriction>
				<owl:onProperty rdf:resource="&fibo-der-drc-bsc;hasUnderlier"/>
				<owl:someValuesFrom rdf:resource="&fibo-der-sbd-sbd;EquityObservable"/>
			</owl:Restriction>
		</rdfs:subClassOf>
		<rdfs:label xml:lang="en">equity dividend swap</rdfs:label>
		<skos:definition xml:lang="en">No definition FpML: Specifies the structure of the dividend swap transaction supplement.</skos:definition>
	</owl:Class>
	
	<owl:Class rdf:about="&fibo-der-sbd-eqs;EquityReturnSwapContract">
		<rdfs:subClassOf rdf:resource="&fibo-der-der-rsw;ReturnSwapContract"/>
		<rdfs:subClassOf rdf:resource="&fibo-der-sbd-sbd;EquityDerivative"/>
		<rdfs:subClassOf>
			<owl:Restriction>
				<owl:onProperty rdf:resource="&fibo-der-drc-bsc;hasUnderlier"/>
				<owl:someValuesFrom rdf:resource="&fibo-der-sbd-sbd;EquityObservable"/>
			</owl:Restriction>
		</rdfs:subClassOf>
		<rdfs:label xml:lang="en">equity return swap contract</rdfs:label>
		<skos:definition xml:lang="en">No definition FpML has no distinct product type for this, instead the schema for Return Swaps has content which is an Equity Swap Transaction Supplement.</skos:definition>
		<fibo-fnd-utl-av:explanatoryNote>The swap itself is typically based on the performance of the security in the marketplace, i.e., the market price.</fibo-fnd-utl-av:explanatoryNote>
	</owl:Class>
	
	<owl:Class rdf:about="&fibo-der-sbd-eqs;EquityVarianceSwapContract">
		<rdfs:subClassOf rdf:resource="&fibo-der-sbd-sbd;EquityDerivative"/>
		<rdfs:subClassOf rdf:resource="&fibo-der-sbd-sbd;StatisticalSwap"/>
		<rdfs:subClassOf>
			<owl:Restriction>
				<owl:onProperty rdf:resource="&fibo-der-drc-bsc;hasUnderlier"/>
				<owl:someValuesFrom rdf:resource="&fibo-der-sbd-sbd;EquityObservable"/>
			</owl:Restriction>
		</rdfs:subClassOf>
		<rdfs:label xml:lang="en">equity variance swap contract</rdfs:label>
		<skos:definition xml:lang="en">no definition FpML (unusable): Specifies the structure of a variance swap.</skos:definition>
	</owl:Class>
	
	<owl:Class rdf:about="&fibo-der-sbd-eqs;SpecialDividendLegTerm">
		<rdfs:label xml:lang="en">special dividend leg term</rdfs:label>
		<skos:definition xml:lang="en">Special dividends and memorial dividends which are applicable. FpML: &apos;If present and true, then special dividends and memorial dividends are applicable.&apos; Note that &quot;if true&quot; (a yes/no term) and &quot;if present&quot; (this term, which is the presence of the thing) are two separate meanings. FpML implies the truth of the Yes/No fact by the presence or absence of this term. However, although FpML definition says &quot;if present and true&quot;, the term is just a &quot;boolean&quot; ie a YTes/no applicability term. Not sure where the special dividends themselves are defined.</skos:definition>
	</owl:Class>
	
	<owl:Class rdf:about="&fibo-der-sbd-eqs;SwapStrikeTerms">
		<rdfs:subClassOf rdf:resource="&fibo-der-drc-swp;SwapLeg"/>
		<rdfs:label xml:lang="en">swap strike terms</rdfs:label>
		<skos:definition xml:lang="en">Formal terms defining the strike leg on a swap that has a strike leg.</skos:definition>
		<fibo-fnd-utl-av:explanatoryNote xml:lang="en">This kind of leg exists for variance swaps and other similar swaps. The realization of this leg is not a cashflow but a netting out against the terms defined in the other leg. Notes from Strike Leg: The abstract leg implied by the strike in a statistical swap. 
Further Notes:This is effectively an abstract leg - there are no streams of payments. Rather, there is one payment on maturity of the contract, which is based on a netting out of this Strike leg and the outcome of the Realized Statistic Leg.</fibo-fnd-utl-av:explanatoryNote>
	</owl:Class>
	
	<owl:Class rdf:about="&fibo-der-sbd-eqs;TotalReturnLeg">
		<rdfs:subClassOf rdf:resource="&fibo-der-der-rsw;AssetReturnStream"/>
		<rdfs:label xml:lang="en">total return leg</rdfs:label>
		<skos:definition xml:lang="en">A leg in which the total return on an asset is paid.</skos:definition>
		<fibo-fnd-utl-av:explanatoryNote xml:lang="en">Used in Total Return Swaps. This is distinguished from the more general Return Leg by the addition of increase or decrease in the value of the underlying asset. General notes from Q2 2010 reviews: Used in the context of credit - have a TRS or a CDS. The difference being: Swap an individeual company&apos;s credit margin vis a vis a reference like basis over libor. Example BHP Billiton&apos;s spread against LIBOR. In contract, with a CDS someone will pay the spread while the other person will only pay in the event of the A default.</fibo-fnd-utl-av:explanatoryNote>
	</owl:Class>
	
	<owl:Class rdf:about="&fibo-der-sbd-eqs;VarianceLegTerms">
		<rdfs:subClassOf rdf:resource="&fibo-der-sbd-sbd;PerformanceBasedVariableLeg"/>
		<rdfs:subClassOf>
			<owl:Restriction>
				<owl:onProperty rdf:resource="&fibo-der-drc-bsc;hasUnderlier"/>
				<owl:someValuesFrom>
					<owl:Restriction>
						<owl:onProperty rdf:resource="&fibo-fnd-rel-rel;hasIdentity"/>
						<owl:someValuesFrom rdf:resource="&fibo-ind-mkt-bas;ReferenceIndex"/>
					</owl:Restriction>
				</owl:someValuesFrom>
			</owl:Restriction>
		</rdfs:subClassOf>
		<rdfs:label xml:lang="en">variance leg terms</rdfs:label>
		<skos:definition xml:lang="en">A return which is driven by a Variance Calculation. Variance of a single price (over time - how is this modeled? Is this the duration of the contract or some defined period or poeriods of time). The variance gets its time basis from the negotiated period in the contract, e.g. Variance over 3 months. Check: Is this always the duration of the contract or can it be for example a set of time scales (say monthly) ove the life of say a 6 month contract, and take an average?? This is logically possible but we don&apos;t know if this is what this is. FpML: A type describing return which is driven by a Variance Calculation. More notes 17 Mar Varianc v covariance Variance is a surrogate for option. Talks about random fluctuation in prices If you look at options theory (black scholes) then the price of an option is 1rily dependent in variation in the price. The more variable the more expensive ot maintain a portfolio that is indifferent to the next move in price. So this Variance Swap allows you to extract that option price (i.e. the variance as above) into the variability of the underlying price. So then the asset being traded is in fact the asset that the price references. context: This is all about controlling the price of an asset (from the point of view of the portfolio holder). similarly with the variance on an index you are picking up on the generic market stability. Recall that an index is controlling an underlying portfolio, but with the index you talk directly about the price (in an index swap), this gives you control of a portfolio that is represented by that index. Basket Swap is this - difference is agreed basket (Index, which has a publisher) versus Basket where the &quot;index&quot; (we don&apos;t call it that here) is a basket of securities.</skos:definition>
	</owl:Class>
	
	<owl:ObjectProperty rdf:about="&fibo-der-sbd-eqs;correlationAmount">
		<rdfs:label xml:lang="en">correlation amount</rdfs:label>
		<rdfs:domain rdf:resource="&fibo-der-sbd-eqs;CorrelationLegTerms"/>
		<rdfs:range rdf:resource="&fibo-fnd-acc-cur;MonetaryAmount"/>
		<skos:definition xml:lang="en">The Equity Amount to which the Equity Payment Date relates in relation to each Equity Payment Date.</skos:definition>
	</owl:ObjectProperty>
	
	<owl:ObjectProperty rdf:about="&fibo-der-sbd-eqs;declaredCashDividendPercentage">
		<rdfs:label xml:lang="en">declared cash dividend percentage</rdfs:label>
		<rdfs:domain rdf:resource="&fibo-der-sbd-eqs;DividendStream"/>
		<rdfs:range rdf:resource="&fibo-fnd-utl-alx;Percentage"/>
		<skos:definition xml:lang="en">The declared Cash Dividend Percentage. FpML: &apos;Declared Cash Dividend Percentage.&apos; Not clear what this means. Action: Move to dated terms.</skos:definition>
	</owl:ObjectProperty>
	
	<owl:ObjectProperty rdf:about="&fibo-der-sbd-eqs;declaredCashEquivalentDividendPercentage">
		<rdfs:label xml:lang="en">declared cash equivalent dividend percentage</rdfs:label>
		<rdfs:domain rdf:resource="&fibo-der-sbd-eqs;DividendStream"/>
		<rdfs:range rdf:resource="&fibo-fnd-utl-alx;Percentage"/>
		<skos:definition xml:lang="en">The declared Cash Equivalent Dividend Percentage. FpML: &apos;Declared Cash Equivalent Dividend Percentage.&apos; This means the equivalent cash value of a divdends paid in kind. Needs terms about how and where abnd by whom the price of those is defined. See &quot;Underlying&quot; relative term. Action: Move to dated terms.</skos:definition>
	</owl:ObjectProperty>
	
	<owl:DatatypeProperty rdf:about="&fibo-der-sbd-eqs;determinationMethod">
		<rdfs:label xml:lang="en">determination method</rdfs:label>
		<rdfs:domain rdf:resource="&fibo-der-sbd-eqs;CorrelationLegTerms"/>
		<skos:definition xml:lang="en">The method according to which an amount or a date is determined.</skos:definition>
	</owl:DatatypeProperty>
	
	<owl:ObjectProperty rdf:about="&fibo-der-sbd-eqs;fixedStrike">
		<rdfs:label xml:lang="en">fixed strike</rdfs:label>
		<rdfs:domain rdf:resource="&fibo-der-sbd-eqs;DividendLegDividendPeriod"/>
		<rdfs:range rdf:resource="&fibo-fnd-acc-cur;MonetaryAmount"/>
		<skos:definition xml:lang="en">The strike amount.</skos:definition>
	</owl:ObjectProperty>
	
	<owl:ObjectProperty rdf:about="&fibo-der-sbd-eqs;hasComponent">
		<rdfs:label xml:lang="en">has component</rdfs:label>
		<rdfs:domain rdf:resource="&fibo-der-sbd-eqs;DividendStream"/>
		<rdfs:range rdf:resource="&fibo-der-sbd-eqs;DividendLegDividendPeriod"/>
	</owl:ObjectProperty>
	
	<owl:ObjectProperty rdf:about="&fibo-der-sbd-eqs;hasComponent.1">
		<rdfs:label xml:lang="en">has component</rdfs:label>
		<rdfs:domain rdf:resource="&fibo-der-sbd-eqs;DividendStream"/>
		<rdfs:range rdf:resource="&fibo-der-sbd-eqs;SpecialDividendLegTerm"/>
	</owl:ObjectProperty>
	
	<owl:ObjectProperty rdf:about="&fibo-der-sbd-eqs;hasSomeDividendPeriods">
		<rdfs:label xml:lang="en">has some dividend periods</rdfs:label>
		<rdfs:domain rdf:resource="&fibo-der-sbd-eqs;DividendLegDividendPeriod"/>
		<rdfs:range rdf:resource="&fibo-der-sbd-eqs;DividendPeriod"/>
	</owl:ObjectProperty>
	
	<owl:DatatypeProperty rdf:about="&fibo-der-sbd-eqs;materialDividendsApplicable">
		<rdfs:label xml:lang="en">material dividends applicable</rdfs:label>
		<rdfs:domain rdf:resource="&fibo-der-sbd-eqs;DividendStream"/>
		<rdfs:range rdf:resource="&xsd;boolean"/>
		<skos:definition xml:lang="en">Whether material non cash dividends are applicable.</skos:definition>
	</owl:DatatypeProperty>
	
	<owl:DatatypeProperty rdf:about="&fibo-der-sbd-eqs;pricingSource">
		<rdfs:label xml:lang="en">pricing source</rdfs:label>
		<rdfs:domain rdf:resource="&fibo-der-sbd-eqs;TotalReturnLeg"/>
	</owl:DatatypeProperty>
	
	<owl:ObjectProperty rdf:about="&fibo-der-sbd-eqs;realizedVarianceAmount">
		<rdfs:label xml:lang="en">realized variance amount</rdfs:label>
		<rdfs:domain rdf:resource="&fibo-der-sbd-eqs;VarianceLegTerms"/>
		<rdfs:range rdf:resource="&fibo-fnd-acc-cur;MonetaryAmount"/>
		<skos:definition xml:lang="en">The amount to which the Equity Payment Date relates, in relation to each Equity Payment Date.</skos:definition>
	</owl:ObjectProperty>
	
	<owl:DatatypeProperty rdf:about="&fibo-der-sbd-eqs;relativeDeterminationMethod">
		<rdfs:label xml:lang="en">relative determination method</rdfs:label>
		<rdfs:domain rdf:resource="&fibo-der-sbd-eqs;CorrelationLegTerms"/>
		<skos:definition xml:lang="en">&apos;A reference to a notional amount determination method defined elsewhere in this document.&apos;</skos:definition>
	</owl:DatatypeProperty>
	
	<owl:DatatypeProperty rdf:about="&fibo-der-sbd-eqs;specialDividendTermsApplicable">
		<rdfs:label xml:lang="en">special dividend terms applicable</rdfs:label>
		<rdfs:domain rdf:resource="&fibo-der-sbd-eqs;DividendStream"/>
		<rdfs:range rdf:resource="&xsd;boolean"/>
		<skos:definition xml:lang="en">Whether special dividends and memorial dividends are applicable. FpML: &apos;If present and true, then special dividends and memorial dividends are applicable.&apos; Note that &quot;if true&quot; (a yes/no term) and &quot;if present&quot; (this term, which is the presence of the thing) are two separate meanings. FpML implies the truth of the Yes/No fact by the presence or absence of the corresponding dividend term.</skos:definition>
	</owl:DatatypeProperty>
	
	<owl:ObjectProperty rdf:about="&fibo-der-sbd-eqs;strike">
		<rdfs:label xml:lang="en">strike</rdfs:label>
		<rdfs:domain rdf:resource="&fibo-der-sbd-eqs;SwapStrikeTerms"/>
		<rdfs:range rdf:resource="&fibo-fnd-acc-cur;MonetaryAmount"/>
		<skos:definition xml:lang="en">The strike amount defined for this leg.</skos:definition>
	</owl:ObjectProperty>

</rdf:RDF>