<?xml version="1.0" encoding="UTF-8"?>
<rdf:RDF xmlns:xsd="http://www.w3.org/2001/XMLSchema#"
         xmlns:sm="http://www.omg.org/techprocess/ab/SpecificationMetadata/"
         xmlns:fibo-fnd-utl-av="http://www.omg.org/spec/EDMC-FIBO/FND/Utilities/AnnotationVocabulary/"
         xmlns:rdf="http://www.w3.org/1999/02/22-rdf-syntax-ns#"
         xmlns:rdfs="http://www.w3.org/2000/01/rdf-schema#"
         xmlns:owl="http://www.w3.org/2002/07/owl#"
         xmlns:skos="http://www.w3.org/2004/02/skos/core#"
         xmlns:dc="http://purl.org/dc/terms/"
         xml:base="http://www.omg.org/spec/EDMC-SR/BE/LegalEntities/CorporateBodies/">

   <owl:Ontology rdf:about="http://www.omg.org/spec/EDMC-SR/BE/LegalEntities/CorporateBodies/">
      <owl:imports rdf:resource="http://www.omg.org/spec/EDMC-SR/BE/LegalEntities/FormalBusinessOrganizations/"/>
      <owl:imports rdf:resource="http://www.omg.org/spec/EDMC-SR/BE/LegalEntities/LegalPersons/"/>
   </owl:Ontology>

   <!--Datatypes-->

<!--Object Properties-->

<owl:ObjectProperty rdf:about="http://www.omg.org/spec/EDMC-SR/BE/LegalEntities/CorporateBodies/bodyCorporateIsConstitutedBy">
      <rdfs:subPropertyOf rdf:resource="http://www.omg.org/spec/EDMC-SR/BE/LegalEntities/CorporateBodies/isConstitutedBy"/>
      <rdfs:domain rdf:resource="http://www.omg.org/spec/EDMC-SR/BE/LegalEntities/CorporateBodies/BodyCorporate"/>
      <rdfs:range rdf:resource="http://www.omg.org/spec/EDMC-SR/BE/LegalEntities/CorporateBodies/InstrumentOfIncorporation"/>
   </owl:ObjectProperty>

   <owl:ObjectProperty rdf:about="http://www.omg.org/spec/EDMC-SR/BE/LegalEntities/CorporateBodies/bodyIncorporatedWithGuaranteeIsGovernedBy">
      <skos:definition>The company is governed by some formal agreement between the principals.</skos:definition>
      <rdfs:subPropertyOf rdf:resource="http://www.omg.org/spec/EDMC-SR/BE/LegalEntities/FormalBusinessOrganizations/formallyConstitutedOrganizationIsGovernedBy"/>
      <rdfs:domain rdf:resource="http://www.omg.org/spec/EDMC-SR/BE/LegalEntities/CorporateBodies/BodyIncorporatedWithGuarantee"/>
      <rdfs:range rdf:resource="http://www.omg.org/spec/EDMC-SR/BE/LegalEntities/CorporateBodies/BodyLimitedByGuaranteePrincipalsAgreement"/>
   </owl:ObjectProperty>

   <owl:ObjectProperty rdf:about="http://www.omg.org/spec/EDMC-SR/BE/LegalEntities/CorporateBodies/guaranteeIsProvidedBy">
      <rdfs:subPropertyOf rdf:resource="http://www.omg.org/spec/EDMC-SR/FND/Relations/Relations/isProvidedBy"/>
      <rdfs:domain rdf:resource="http://www.omg.org/spec/EDMC-SR/BE/LegalEntities/CorporateBodies/IncorporationGuarantee"/>
      <rdfs:range rdf:resource="http://www.omg.org/spec/EDMC-SR/FND/Relations/Relations/Thing"/>
   </owl:ObjectProperty>

   <owl:ObjectProperty rdf:about="http://www.omg.org/spec/EDMC-SR/BE/LegalEntities/CorporateBodies/incorporationGuaranteeHasNotionalAmount">
      <rdfs:subPropertyOf rdf:resource="http://www.omg.org/spec/FIBO/Foundation/Accounting/CurrencyAmount/hasNotionalAmount"/>
      <rdfs:domain rdf:resource="http://www.omg.org/spec/EDMC-SR/BE/LegalEntities/CorporateBodies/IncorporationGuarantee"/>
      <rdfs:range rdf:resource="http://www.omg.org/spec/FIBO/Foundation/Accounting/CurrencyAmount/MonetaryAmount"/>
   </owl:ObjectProperty>

   <owl:ObjectProperty rdf:about="http://www.omg.org/spec/EDMC-SR/BE/LegalEntities/CorporateBodies/instrumentOfIncorporationIsGovernedBy">
      <skos:definition>The legal jurisdiction under which the Instrument of Incorporation has standing.</skos:definition>
      <rdfs:subPropertyOf rdf:resource="http://www.omg.org/spec/EDMC-SR/FND/Relations/Relations/isGoverneBy"/>
      <rdfs:domain rdf:resource="http://www.omg.org/spec/EDMC-SR/BE/LegalEntities/CorporateBodies/InstrumentOfIncorporation"/>
      <rdfs:range rdf:resource="http://www.omg.org/spec/EDMC-SR/FND/Law/Jurisdictions/Jurisdiction"/>
   </owl:ObjectProperty>

   <owl:ObjectProperty rdf:about="http://www.omg.org/spec/EDMC-SR/BE/LegalEntities/CorporateBodies/isConstitutedBy">
      <skos:definition>The instrument by which the entity is incorporated.</skos:definition>
      <rdfs:domain rdf:resource="http://www.omg.org/spec/EDMC-SR/BE/LegalEntities/CorporateBodies/BodyCorporate"/>
      <rdfs:range rdf:resource="http://www.omg.org/spec/EDMC-SR/FND/Law/LegalCore/Constitution"/>
   </owl:ObjectProperty>

   <owl:ObjectProperty rdf:about="http://www.omg.org/spec/EDMC-SR/BE/LegalEntities/CorporateBodies/isDomiciledIn">
      <skos:definition>The country in which the Body Corporate is officially domiciled.</skos:definition>
      <skos:editorialNote>This would normally be the country corresponding to the Jurisdiction in which the Body Corporate is incorporated. For some, primarily federal countries, the Domicile is the country that makes up the federation while the Jurisdiction under which the entity is registered would be that of some state in that federation.</skos:editorialNote>
      <rdfs:domain rdf:resource="http://www.omg.org/spec/EDMC-SR/BE/LegalEntities/CorporateBodies/BodyCorporate"/>
      <rdfs:range rdf:resource="http://www.omg.org/spec/EDMC-SR/FND/Places/Countries/Country"/>
   </owl:ObjectProperty>

   <owl:ObjectProperty rdf:about="http://www.omg.org/spec/EDMC-SR/BE/LegalEntities/CorporateBodies/isIncorporatedIn">
      <skos:definition>The legal jurisdiction under which the legal entity is incorporated.</skos:definition>
      <skos:editorialNote>It is the laws of this jurisdiction that cause and allow the legal entity to exist and to incur debt and be sued at law as a legal entity.</skos:editorialNote>
      <rdfs:domain rdf:resource="http://www.omg.org/spec/EDMC-SR/BE/LegalEntities/CorporateBodies/BodyCorporate"/>
      <rdfs:range rdf:resource="http://www.omg.org/spec/EDMC-SR/FND/Law/Jurisdictions/Jurisdiction"/>
   </owl:ObjectProperty>

   <owl:ObjectProperty rdf:about="http://www.omg.org/spec/EDMC-SR/BE/LegalEntities/CorporateBodies/issuesEquity">
      <skos:definition>The Body Incorporated by Equity is incorporated through the issuance of some Issued Equity, which is a form of Stockholder Equity.</skos:definition>
      <rdfs:subPropertyOf rdf:resource="http://www.omg.org/spec/EDMC-SR/BE/LegalEntities/FormalBusinessOrganizations/hasEquity"/>
      <rdfs:domain rdf:resource="http://www.omg.org/spec/EDMC-SR/BE/LegalEntities/CorporateBodies/BodyIncorporatedWithEquity"/>
      <rdfs:range rdf:resource="http://www.omg.org/spec/EDMC-SR/FND/Accounting/AccountingEquity/IssuedEquity"/>
   </owl:ObjectProperty>

   <!--Data Properties-->

<owl:DatatypeProperty rdf:about="http://www.omg.org/spec/EDMC-SR/BE/LegalEntities/CorporateBodies/hasLegalName">
      <rdfs:range rdf:resource="http://www.omg.org/spec/EDMC-SR/FND/Utilities/BusinessFacingTypes/text"/>
   </owl:DatatypeProperty>

   <owl:DatatypeProperty rdf:about="http://www.omg.org/spec/EDMC-SR/BE/LegalEntities/CorporateBodies/instrumentURI">
      <rdfs:range rdf:resource="http://www.omg.org/spec/EDMC-SR/FND/Utilities/BusinessFacingTypes/URI"/>
   </owl:DatatypeProperty>

   <!--Annotation Properties-->

<!--Classes-->

<owl:Class rdf:about="http://www.omg.org/spec/EDMC-SR/BE/LegalEntities/CorporateBodies/BodyCorporate">
      <rdfs:label>Body Corporate</rdfs:label>
      <skos:definition>Any formal organization which can incur liability and can be sued at law and which is not an individual human being.</skos:definition>
      <skos:editorialNote>This is an artificial legal person, that is something with legal personhood but which has been created artificially. It is also a formal organization (unlike for example artificial legal persons created by statute br by royal charter). Bodies Corporate, and all non natural legal persons, are generally created by some legal act and supported by some instrument such as the issuance of shares or guarantees. These are what give the entity a separate legal standing in the jurisdiction in which they are defined, and that jurisdiction will have created the laws which allow and cause this kind of entity to exist.</skos:editorialNote>
      <rdfs:subClassOf rdf:resource="http://www.omg.org/spec/EDMC-SR/BE/LegalEntities/LegalPersons/JudicialPerson"/>
      <rdfs:subClassOf rdf:resource="http://www.omg.org/spec/EDMC-SR/BE/LegalEntities/FormalBusinessOrganizations/FormallyConstitutedOrganization"/>
   </owl:Class>

   <owl:Class rdf:about="http://www.omg.org/spec/EDMC-SR/BE/LegalEntities/CorporateBodies/BodyIncorporatedThroughAgreement">
      <rdfs:label>Body Incorporated Through Agreement</rdfs:label>
      <skos:definition>A body with legal personhood, incorporated through some agreement among the principals, and without equity or guarantee instruments which would isolate the principals from liability.</skos:definition>
      <skos:editorialNote>An LLP (in the UK) is an example of this, and is also a partnership. There, the LLP Document is the legal document which effectively constitutes the Partnership.</skos:editorialNote>
      <rdfs:subClassOf rdf:resource="http://www.omg.org/spec/EDMC-SR/BE/LegalEntities/CorporateBodies/BodyCorporate"/>
   </owl:Class>

   <owl:Class rdf:about="http://www.omg.org/spec/EDMC-SR/BE/LegalEntities/CorporateBodies/BodyIncorporatedWithEquity">
      <rdfs:label>Body Incorporated With Equity</rdfs:label>
      <skos:definition>A body corporate which is incorporated by means of the issuance of equity.</skos:definition>
   </owl:Class>

   <owl:Class rdf:about="http://www.omg.org/spec/EDMC-SR/BE/LegalEntities/CorporateBodies/BodyIncorporatedWithGuarantee">
      <rdfs:label>Body Incorporated With Guarantee</rdfs:label>
   </owl:Class>

   <owl:Class rdf:about="http://www.omg.org/spec/EDMC-SR/BE/LegalEntities/CorporateBodies/BodyLimitedByGuaranteePrincipalsAgreement">
      <rdfs:label>Body Limited By Guarantee Principals Agreement</rdfs:label>
      <skos:definition>The formal agreement between the principals of a Body Limited by Guarantee.</skos:definition>
      <rdfs:subClassOf rdf:resource="http://www.omg.org/spec/EDMC-SR/BE/LegalEntities/FormalBusinessOrganizations/OrganizationCoveringAgreement"/>
   </owl:Class>

   <owl:Class rdf:about="http://www.omg.org/spec/EDMC-SR/BE/LegalEntities/CorporateBodies/CompanyIncorporatedByGuarantee">
      <rdfs:label>Company Incorporated By Guarantee</rdfs:label>
      <rdfs:subClassOf rdf:resource="http://www.omg.org/spec/EDMC-SR/BE/LegalEntities/CorporateBodies/BodyIncorporatedWithGuarantee"/>
   </owl:Class>

   <owl:Class rdf:about="http://www.omg.org/spec/EDMC-SR/BE/LegalEntities/CorporateBodies/IncorporationGuarantee">
      <rdfs:label>Incorporation Guarantee</rdfs:label>
      <skos:definition>A guarantee which is part of the means by which some incorporated entity is incorporated by guarantee.</skos:definition>
      <rdfs:subClassOf rdf:resource="http://www.omg.org/spec/EDMC-SR/FND/Law/LegalCore/Constitution"/>
   </owl:Class>

   <owl:Class rdf:about="http://www.omg.org/spec/EDMC-SR/BE/LegalEntities/CorporateBodies/InstrumentOfIncorporation">
      <rdfs:label>Instrument Of Incorporation</rdfs:label>
      <skos:definition>Some legal instrument by which some legal entity which is not a natural person is made to exist.</skos:definition>
      <skos:editorialNote>This may be the issuance of shares, the existence of some agreement, guaranties and so on.</skos:editorialNote>
   </owl:Class>

   <!--Individuals-->

</rdf:RDF>