<?xml version="1.0" encoding="UTF-8"?>
  
<!DOCTYPE rdf:RDF [
    <!ENTITY fibo-sec-dbt-bond-strip "http://spec.edmcouncil.org/fibo/red/sec/debt/bonds/strips/">
    <!ENTITY fibo-sec-dbt-dbt-ins "http://spec.edmcouncil.org/fibo/red/sec/debt/debt-foundations/debt-instruments/">
    <!ENTITY fibo-sec-dbt-bond-bond "http://spec.edmcouncil.org/fibo/red/sec/debt/bonds/bonds-common/">
    <!ENTITY fibo-fnd-utl-bt "http://spec.edmcouncil.org/fibo/red/fnd/utilities/business-facing-types/">
]>

<rdf:RDF xmlns:xsd="http://www.w3.org/2001/XMLSchema#"
         xmlns:sm="http://www.omg.org/techprocess/ab/SpecificationMetadata/"
         xmlns:xs="http://www.w3.org/2001/XMLSchema"
         xmlns:fibo-fnd-utl-av="http://www.omg.org/spec/EDMC-FIBO/FND/Utilities/AnnotationVocabulary/"
         xmlns:rdf="http://www.w3.org/1999/02/22-rdf-syntax-ns#"
         xmlns:rdfs="http://www.w3.org/2000/01/rdf-schema#"
         xmlns:owl="http://www.w3.org/2002/07/owl#"
         xmlns:skos="http://www.w3.org/2004/02/skos/core#"
         xmlns:dc="http://purl.org/dc/terms/"
         xml:base="http://spec.edmcouncil.org/fibo/red/sec/debt/bonds/strips/">

   <owl:Ontology rdf:about="http://spec.edmcouncil.org/fibo/red/sec/debt/bonds/strips/">
      <owl:imports rdf:resource="http://spec.edmcouncil.org/fibo/red/sec/debt/debt-foundations/debt-instruments/"/>
      <owl:imports rdf:resource="http://spec.edmcouncil.org/fibo/red/sec/debt/bonds/bonds-common/"/>
      <owl:imports rdf:resource="http://spec.edmcouncil.org/fibo/red/fnd/utilities/business-facing-types/"/>
   </owl:Ontology>


  <!--
    ///////////////////////////////////////////////////////////////////////////////////////
    //
    // Datatypes
    //
    ///////////////////////////////////////////////////////////////////////////////////////
    -->



  <!--
    ///////////////////////////////////////////////////////////////////////////////////////
    //
    // Object Properties
    //
    ///////////////////////////////////////////////////////////////////////////////////////
    -->


<owl:ObjectProperty rdf:about="&fibo-sec-dbt-bond-strip;isStripOfUnderlying">
      <rdfs:label>is strip of underlying</rdfs:label>
      <rdfs:domain rdf:resource="&fibo-sec-dbt-bond-strip;STRIP"/>
      <rdfs:range rdf:resource="&fibo-sec-dbt-bond-bond;Bond"/>
   </owl:ObjectProperty>


  <!--
    ///////////////////////////////////////////////////////////////////////////////////////
    //
    // Data Properties
    //
    ///////////////////////////////////////////////////////////////////////////////////////
    -->


<owl:DatatypeProperty rdf:about="&fibo-sec-dbt-bond-strip;interestStrip">
      <rdfs:label>interest strip</rdfs:label>
      <skos:definition>The STRIP instrument is a strip of the Interest of the underlying Debt Instrument.</skos:definition>
      <rdfs:range rdf:resource="&fibo-fnd-utl-bt;yesOrNo"/>
   </owl:DatatypeProperty>

   <owl:DatatypeProperty rdf:about="&fibo-sec-dbt-bond-strip;principalStrip">
      <rdfs:label>principal strip</rdfs:label>
      <skos:definition>The STRIP instrument is not a strip of the Principal of the underlying Debt Instrument.</skos:definition>
      <rdfs:range rdf:resource="&fibo-fnd-utl-bt;yesOrNo"/>
   </owl:DatatypeProperty>

   <owl:DatatypeProperty rdf:about="&fibo-sec-dbt-bond-strip;interestStrip.1">
      <rdfs:label>interest strip</rdfs:label>
      <skos:definition>The STRIP instrument is not a strip of the Interest of the underlying Debt Instrument.</skos:definition>
      <rdfs:range rdf:resource="&fibo-fnd-utl-bt;yesOrNo"/>
   </owl:DatatypeProperty>

   <owl:DatatypeProperty rdf:about="&fibo-sec-dbt-bond-strip;principalStrip.1">
      <rdfs:label>principal strip</rdfs:label>
      <skos:definition>The STRIP instrument is a strip of the Principal of the underlying Debt Instrument.</skos:definition>
      <rdfs:range rdf:resource="&fibo-fnd-utl-bt;yesOrNo"/>
   </owl:DatatypeProperty>

   <owl:DatatypeProperty rdf:about="&fibo-sec-dbt-bond-strip;interestStrip.2">
      <rdfs:label>interest strip</rdfs:label>
      <skos:definition>Whether the STRIP instrument is a strip of the Interest of the underlying Debt Instrument.</skos:definition>
      <rdfs:range rdf:resource="&fibo-fnd-utl-bt;yesOrNo"/>
   </owl:DatatypeProperty>

   <owl:DatatypeProperty rdf:about="&fibo-sec-dbt-bond-strip;principalStrip.2">
      <rdfs:label>principal strip</rdfs:label>
      <skos:definition>Whether the STRIP instrument is a strip of the Principal of the underlying Debt Instrument.</skos:definition>
      <rdfs:range rdf:resource="&fibo-fnd-utl-bt;yesOrNo"/>
   </owl:DatatypeProperty>


  <!--
    ///////////////////////////////////////////////////////////////////////////////////////
    //
    // Annotation Properties
    //
    ///////////////////////////////////////////////////////////////////////////////////////
    -->



  <!--
    ///////////////////////////////////////////////////////////////////////////////////////
    //
    // Classes
    //
    ///////////////////////////////////////////////////////////////////////////////////////
    -->


<owl:Class rdf:about="&fibo-sec-dbt-bond-strip;InterestSTRIP">
      <rdfs:label>interest s t r i p</rdfs:label>
      <skos:definition>A Debt Instrument which consists of the interest component alone, of a Debt Security.</skos:definition>
      <rdfs:subClassOf rdf:resource="&fibo-sec-dbt-bond-strip;STRIP"/>
   </owl:Class>

   <owl:Class rdf:about="&fibo-sec-dbt-bond-strip;PrincipalSTRIP">
      <rdfs:label>principal s t r i p</rdfs:label>
      <skos:definition>A Debt Instrument which consists of the principal component alone, of a Debt Security.</skos:definition>
   </owl:Class>

   <owl:Class rdf:about="&fibo-sec-dbt-bond-strip;STRIP">
      <rdfs:label>s t r i p</rdfs:label>
      <skos:definition>Separate Trading of Registered Interest and Principal of Securities. A Debt Instrument which consists of either the interest component alone, or the principal component alone, of a bond.</skos:definition>
      <rdfs:subClassOf rdf:resource="&fibo-sec-dbt-dbt-ins;TradableDebtInstrument"/>
   </owl:Class>


  <!--
    ///////////////////////////////////////////////////////////////////////////////////////
    //
    // Individuals
    //
    ///////////////////////////////////////////////////////////////////////////////////////
    -->


</rdf:RDF>