<?xml version="1.0" encoding="UTF-8"?>
<rdf:RDF xmlns:xsd="http://www.w3.org/2001/XMLSchema#"
         xmlns:sm="http://www.omg.org/techprocess/ab/SpecificationMetadata/"
         xmlns:fibo-fnd-utl-av="http://www.omg.org/spec/EDMC-FIBO/FND/Utilities/AnnotationVocabulary/"
         xmlns:rdf="http://www.w3.org/1999/02/22-rdf-syntax-ns#"
         xmlns:rdfs="http://www.w3.org/2000/01/rdf-schema#"
         xmlns:owl="http://www.w3.org/2002/07/owl#"
         xmlns:skos="http://www.w3.org/2004/02/skos/core#"
         xmlns:dc="http://purl.org/dc/terms/"
         xml:base="http://www.omg.org/spec/EDMC-SR/BE/OwnershipAndControl/ControlParties/">

   <owl:Ontology rdf:about="http://www.omg.org/spec/EDMC-SR/BE/OwnershipAndControl/ControlParties/">
      <owl:imports rdf:resource="http://www.omg.org/spec/EDMC-SR/BE/OwnershipAndControl/OwnershipParties/"/>
      <owl:imports rdf:resource="http://www.omg.org/spec/EDMC-SR/FND/OwnershipAndControl/Control/"/>
   </owl:Ontology>

   <!--Datatypes-->

<!--Object Properties-->

<owl:ObjectProperty rdf:about="http://www.omg.org/spec/EDMC-SR/BE/OwnershipAndControl/ControlParties/constitutionalContractualControlIsConferredBy">
      <skos:definition>The control is conferred on the party by means of the formal covering agreement by which the organization is constituted, that is the agreement between the principals of the organization.</skos:definition>
      <rdfs:subPropertyOf rdf:resource="http://www.omg.org/spec/EDMC-SR/BE/OwnershipAndControl/ControlParties/contractualControlIsConferredBy"/>
      <rdfs:domain rdf:resource="http://www.omg.org/spec/EDMC-SR/BE/OwnershipAndControl/ControlParties/ConstitutionalContractualControl"/>
      <rdfs:range rdf:resource="http://www.omg.org/spec/EDMC-SR/BE/LegalEntities/FormalBusinessOrganizations/OrganizationCoveringAgreement"/>
   </owl:ObjectProperty>

   <owl:ObjectProperty rdf:about="http://www.omg.org/spec/EDMC-SR/BE/OwnershipAndControl/ControlParties/contractualControlIsConferredBy">
      <skos:definition>The control is conferred on the party by means of some contract.</skos:definition>
      <rdfs:subPropertyOf rdf:resource="http://www.omg.org/spec/EDMC-SR/FND/Law/LegalCapacities/isConferredBy"/>
      <rdfs:domain rdf:resource="http://www.omg.org/spec/EDMC-SR/BE/OwnershipAndControl/ControlParties/ContractualControl"/>
      <rdfs:range rdf:resource="http://www.omg.org/spec/EDMC-SR/FND/Agreements/Contracts/Contract"/>
   </owl:ObjectProperty>

   <owl:ObjectProperty rdf:about="http://www.omg.org/spec/EDMC-SR/BE/OwnershipAndControl/ControlParties/controlledPartyIsControlledToSomeDegreeBy">
      <rdfs:subPropertyOf rdf:resource="http://www.omg.org/spec/EDMC-SR/BE/OwnershipAndControl/ControlParties/isControlledToSomeDegreeBy"/>
      <rdfs:domain rdf:resource="http://www.omg.org/spec/EDMC-SR/BE/OwnershipAndControl/ControlParties/ControlledParty"/>
      <rdfs:range rdf:resource="http://www.omg.org/spec/EDMC-SR/FND/AgentsAndPeople/Agents/AutonomousAgent"/>
   </owl:ObjectProperty>

   <owl:ObjectProperty rdf:about="http://www.omg.org/spec/EDMC-SR/BE/OwnershipAndControl/ControlParties/courtAppoinredControlIsConferredBy">
      <skos:definition>The control which is vested in the controlling party is conferred upon that party through some court of law.</skos:definition>
      <rdfs:subPropertyOf rdf:resource="http://www.omg.org/spec/EDMC-SR/FND/Law/LegalCapacities/isConferredBy"/>
      <rdfs:domain rdf:resource="http://www.omg.org/spec/EDMC-SR/BE/OwnershipAndControl/ControlParties/CourtAppointedControl"/>
      <rdfs:range rdf:resource="http://www.omg.org/spec/EDMC-SR/FND/Law/LegalCore/CourtOfLaw"/>
   </owl:ObjectProperty>

   <owl:ObjectProperty rdf:about="http://www.omg.org/spec/EDMC-SR/BE/OwnershipAndControl/ControlParties/jointControllingPartyIdentity">
      <skos:definition>The identity of the Party is some group of entities which have formed some alliance or agreement in terms of which they jointly exercise control over the controlled organization.</skos:definition>
      <rdfs:subPropertyOf rdf:resource="http://www.omg.org/spec/EDMC-SR/FND/Parties/Parties/partyInRoleHasIdentity"/>
      <rdfs:domain rdf:resource="http://www.omg.org/spec/EDMC-SR/BE/OwnershipAndControl/ControlParties/JointControllingParty"/>
      <rdfs:range rdf:resource="http://www.omg.org/spec/EDMC-SR/BE/OwnershipAndControl/ControlParties/ControllingAlliance"/>
   </owl:ObjectProperty>

   <owl:ObjectProperty rdf:about="http://www.omg.org/spec/EDMC-SR/BE/OwnershipAndControl/ControlParties/limitedControllingPartyHasNatureOControl">
      <skos:definition>The type of control for which the party has the stated percentage.</skos:definition>
      <skos:editorialNote>Assertions or analysis may produce the result that a given entity is said to assert a percentage of some control - this is necessarily defined as a percentage of a given kind of control, defined in terms of a given kind of activity which the controlled entity may be made to perform on the basis of that control. This relationship defines the type of control in question.</skos:editorialNote>
      <rdfs:subPropertyOf rdf:resource="http://www.omg.org/spec/EDMC-SR/BE/OwnershipAndControl/ControlParties/exercisesSomeDegreeOf"/>
      <rdfs:domain rdf:resource="http://www.omg.org/spec/EDMC-SR/BE/OwnershipAndControl/ControlParties/LimitedControllingParty"/>
      <rdfs:range rdf:resource="http://www.omg.org/spec/EDMC-SR/BE/OwnershipAndControl/ControlParties/LimitedDeFactoControl"/>
   </owl:ObjectProperty>

   <owl:ObjectProperty rdf:about="http://www.omg.org/spec/EDMC-SR/BE/OwnershipAndControl/ControlParties/exercisesContractualControl">
      <skos:definition>Control is exercised by the party, which is conferred by some contractual agreement.</skos:definition>
      <rdfs:subPropertyOf rdf:resource="http://www.omg.org/spec/EDMC-SR/BE/OwnershipAndControl/ControlParties/holdsSomeInstrumentOfDeJureControl"/>
      <rdfs:domain rdf:resource="http://www.omg.org/spec/EDMC-SR/BE/OwnershipAndControl/ControlParties/ContractualControllingParty"/>
      <rdfs:range rdf:resource="http://www.omg.org/spec/EDMC-SR/BE/OwnershipAndControl/ControlParties/ContractualControl"/>
   </owl:ObjectProperty>

   <owl:ObjectProperty rdf:about="http://www.omg.org/spec/EDMC-SR/BE/OwnershipAndControl/ControlParties/exercisesCourtAppointedControl">
      <skos:definition>Legal control exercised by the party, which is appointed by some court.</skos:definition>
      <skos:editorialNote>Typically as a result of bankruptcy action.</skos:editorialNote>
      <rdfs:subPropertyOf rdf:resource="http://www.omg.org/spec/EDMC-SR/BE/OwnershipAndControl/ControlParties/holdsSomeInstrumentOfDeJureControl"/>
      <rdfs:domain rdf:resource="http://www.omg.org/spec/EDMC-SR/BE/OwnershipAndControl/ControlParties/Receiver"/>
      <rdfs:range rdf:resource="http://www.omg.org/spec/EDMC-SR/BE/OwnershipAndControl/ControlParties/CourtAppointedControl"/>
   </owl:ObjectProperty>

   <owl:ObjectProperty rdf:about="http://www.omg.org/spec/EDMC-SR/BE/OwnershipAndControl/ControlParties/exercisesInvestmentBasedDeFactoControl">
      <skos:definition>The party exercises some degree of de facto control based on some investment which they hold in the entity.</skos:definition>
      <rdfs:subPropertyOf rdf:resource="http://www.omg.org/spec/EDMC-SR/BE/OwnershipAndControl/ControlParties/holdsSomeMeansOfDeFactoControl"/>
      <rdfs:domain rdf:resource="http://www.omg.org/spec/EDMC-SR/BE/OwnershipAndControl/ControlParties/InvestmentBasedDeFactoControllingInterestParty"/>
      <rdfs:range rdf:resource="http://www.omg.org/spec/EDMC-SR/BE/OwnershipAndControl/ControlParties/InvestmentBasedDeFactoControl"/>
   </owl:ObjectProperty>

   <owl:ObjectProperty rdf:about="http://www.omg.org/spec/EDMC-SR/BE/OwnershipAndControl/ControlParties/hasSignificantControllingInterstParty">
      <skos:definition>Some entity which owns a significant part of this company but not 50% or more.</skos:definition>
      <skos:editorialNote>This is a relationship for "any" ownership between a lower threshold (defined in AML regulations locally) and 50%. It is the inverse of the Affiliate (AKA Associate) relationship.</skos:editorialNote>
      <rdfs:subPropertyOf rdf:resource="http://www.edmcouncil.org/spec/EDMC-SR/BE/OwnershipAndControlExt/ControlPartiesExtras/hasDeJureControllingInterestParty"/>
      <rdfs:subPropertyOf rdf:resource="http://www.omg.org/spec/EDMC-SR/BE/OwnershipAndControl/ControlParties/hasControllingInterestParty"/>
      <rdfs:domain rdf:resource="http://www.omg.org/spec/EDMC-SR/BE/LegalEntities/FormalBusinessOrganizations/FormallyConstitutedOrganization"/>
      <rdfs:range rdf:resource="http://www.omg.org/spec/EDMC-SR/BE/OwnershipAndControl/ControlParties/SignificantControllingInterestParty"/>
   </owl:ObjectProperty>

   <owl:ObjectProperty rdf:about="http://www.omg.org/spec/EDMC-SR/BE/OwnershipAndControl/ControlParties/hasTotalOwner">
      <skos:definition>The Formal Organization is totally owned and therefore wholly controlled by some party having 100% ownership in it.</skos:definition>
      <skos:editorialNote>This may be any entity which is capable of exercising ownership. Scope Note: By virtue of holding 100% of the equity ownership, the Total Owner also holds 100% of the controlling equity, if there is a difference. Therefore it is both a total owner and a total controlling party. For this reason it is included among the control relationships and is a specialization of the "has majority controlling party" relationships.</skos:editorialNote>
      <rdfs:subPropertyOf rdf:resource="http://www.omg.org/spec/EDMC-SR/BE/OwnershipAndControl/OwnershipParties/hasConstitutionalOwner"/>
      <rdfs:domain rdf:resource="http://www.omg.org/spec/EDMC-SR/BE/LegalEntities/FormalBusinessOrganizations/FormallyConstitutedOrganization"/>
      <rdfs:range rdf:resource="http://www.omg.org/spec/EDMC-SR/BE/OwnershipAndControl/ControlParties/TotalOwner"/>
   </owl:ObjectProperty>

   <owl:ObjectProperty rdf:about="http://www.omg.org/spec/EDMC-SR/BE/OwnershipAndControl/ControlParties/hasControllingInterestParty">
      <skos:definition>The Formal Organization is controlled in some way by some controlling party, that is some entity which exercises such control.</skos:definition>
      <rdfs:subPropertyOf rdf:resource="http://www.omg.org/spec/EDMC-SR/FND/Parties/Parties/hasPartyInRole"/>
      <rdfs:domain rdf:resource="http://www.omg.org/spec/EDMC-SR/BE/LegalEntities/FormalBusinessOrganizations/FormallyConstitutedOrganization"/>
      <rdfs:range rdf:resource="http://www.omg.org/spec/EDMC-SR/BE/OwnershipAndControl/ControlParties/ControllingInterestParty"/>
   </owl:ObjectProperty>

   <owl:ObjectProperty rdf:about="http://www.omg.org/spec/EDMC-SR/BE/OwnershipAndControl/ControlParties/hasDegreeOfControl">
      <skos:definition>has degree of control, (partial, majority, or complete) either alone or with other parties, with respect to some activity</skos:definition>
      <rdfs:domain rdf:resource="http://www.omg.org/spec/EDMC-SR/BE/OwnershipAndControl/ControlParties/EntityControllingParty"/>
      <rdfs:range rdf:resource="http://www.omg.org/spec/EDMC-SR/BE/OwnershipAndControl/ControlParties/DegreeOfControl"/>
   </owl:ObjectProperty>

   <owl:ObjectProperty rdf:about="http://www.omg.org/spec/EDMC-SR/BE/OwnershipAndControl/ControlParties/hasMajorityControllingParty">
      <skos:definition>The parent of the company, if there is one.</skos:definition>
      <skos:editorialNote>This is usually (but not necessarily) any entity which owns a controlling stake of &amp;gt;50% (50% plus one voting share or above, or equivalent) in this company, if it is a limited company.</skos:editorialNote>
      <rdfs:subPropertyOf rdf:resource="http://www.omg.org/spec/EDMC-SR/BE/OwnershipAndControl/ControlParties/isControlledToSomeDegreeBy"/>
      <rdfs:domain rdf:resource="http://www.omg.org/spec/EDMC-SR/BE/LegalEntities/FormalBusinessOrganizations/FormallyConstitutedOrganization"/>
      <rdfs:range rdf:resource="http://www.omg.org/spec/EDMC-SR/BE/OwnershipAndControl/ControlParties/MajorityControllingParty"/>
   </owl:ObjectProperty>

   <owl:ObjectProperty rdf:about="http://www.omg.org/spec/EDMC-SR/BE/OwnershipAndControl/ControlParties/exercisesSomeDegreeOf">
      <skos:definition>has nature or kind of control, de facto or limited de facto control</skos:definition>
      <rdfs:domain rdf:resource="http://www.omg.org/spec/EDMC-SR/BE/OwnershipAndControl/ControlParties/EntityControllingParty"/>
      <rdfs:range rdf:resource="http://www.omg.org/spec/EDMC-SR/FND/OwnershipAndControl/Control/DeFactoControl"/>
   </owl:ObjectProperty>

   <owl:ObjectProperty rdf:about="http://www.omg.org/spec/EDMC-SR/BE/OwnershipAndControl/ControlParties/exercisesSomeInvestmentBasedDeFactoControl">
      <skos:definition>The party exercises some de facto control based on some investment in equity.</skos:definition>
      <rdfs:subPropertyOf rdf:resource="http://www.omg.org/spec/EDMC-SR/BE/OwnershipAndControl/ControlParties/holdsSomeMeansOfDeFactoControl"/>
      <rdfs:domain rdf:resource="http://www.omg.org/spec/EDMC-SR/BE/OwnershipAndControl/ControlParties/ControllingLeverageParty"/>
      <rdfs:range rdf:resource="http://www.omg.org/spec/EDMC-SR/BE/OwnershipAndControl/ControlParties/InvestmentBasedDeFactoControl"/>
   </owl:ObjectProperty>

   <owl:ObjectProperty rdf:about="http://www.omg.org/spec/EDMC-SR/BE/OwnershipAndControl/ControlParties/holdsSomeInstrumentOfDeJureControl">
      <skos:definition>Legal or contractually based control exercised by the party.</skos:definition>
      <rdfs:subPropertyOf rdf:resource="http://www.omg.org/spec/EDMC-SR/BE/OwnershipAndControl/ControlParties/holdsSomeMeansOf"/>
      <rdfs:domain rdf:resource="http://www.omg.org/spec/EDMC-SR/BE/OwnershipAndControl/ControlParties/DeJureControllingInterestParty"/>
      <rdfs:range rdf:resource="http://www.omg.org/spec/EDMC-SR/BE/OwnershipAndControl/ControlParties/DeJureControllingInterest"/>
   </owl:ObjectProperty>

   <owl:ObjectProperty rdf:about="http://www.omg.org/spec/EDMC-SR/BE/OwnershipAndControl/ControlParties/holdsSomeMeansOfDeFactoControl">
      <skos:definition>The party exercises some control which is not based in law or contract but in some other means.</skos:definition>
      <rdfs:subPropertyOf rdf:resource="http://www.omg.org/spec/EDMC-SR/BE/OwnershipAndControl/ControlParties/holdsSomeMeansOf"/>
      <rdfs:domain rdf:resource="http://www.omg.org/spec/EDMC-SR/BE/OwnershipAndControl/ControlParties/DeFactoControllingInterestParty"/>
      <rdfs:range rdf:resource="http://www.omg.org/spec/EDMC-SR/FND/OwnershipAndControl/Control/DeFactoControl"/>
   </owl:ObjectProperty>

   <owl:ObjectProperty rdf:about="http://www.omg.org/spec/EDMC-SR/BE/OwnershipAndControl/ControlParties/exercisesSomeInfluenceBasedDeFactoControl">
      <skos:definition>Exercises some influence and control other than by means of investment.</skos:definition>
      <rdfs:subPropertyOf rdf:resource="http://www.omg.org/spec/EDMC-SR/BE/OwnershipAndControl/ControlParties/holdsSomeMeansOfDeFactoControl"/>
      <rdfs:domain rdf:resource="http://www.omg.org/spec/EDMC-SR/BE/OwnershipAndControl/ControlParties/InfluenceBasedDeFactoControllingParty"/>
      <rdfs:range rdf:resource="http://www.omg.org/spec/EDMC-SR/BE/OwnershipAndControl/ControlParties/InfluenceBasedDeFactoControl"/>
   </owl:ObjectProperty>

   <owl:ObjectProperty rdf:about="http://www.omg.org/spec/EDMC-SR/BE/OwnershipAndControl/ControlParties/holdsTheOptionToExercise">
      <skos:definition>Control which may optionally be exercised by the party.</skos:definition>
      <rdfs:subPropertyOf rdf:resource="http://www.omg.org/spec/EDMC-SR/BE/OwnershipAndControl/ControlParties/holdsSomeMeansOf"/>
      <rdfs:domain rdf:resource="http://www.omg.org/spec/EDMC-SR/BE/OwnershipAndControl/ControlParties/PartyHoldingSomeOptionForControl"/>
      <rdfs:range rdf:resource="http://www.omg.org/spec/EDMC-SR/BE/OwnershipAndControl/ControlParties/DeJureControllingInterest"/>
   </owl:ObjectProperty>

   <owl:ObjectProperty rdf:about="http://www.omg.org/spec/EDMC-SR/BE/OwnershipAndControl/ControlParties/holdsSomeMeansOf">
      <skos:definition>Some means of control held by the party.</skos:definition>
      <rdfs:domain rdf:resource="http://www.omg.org/spec/EDMC-SR/BE/OwnershipAndControl/ControlParties/ControllingInterestParty"/>
      <rdfs:range rdf:resource="http://www.omg.org/spec/EDMC-SR/FND/OwnershipAndControl/Control/Control"/>
   </owl:ObjectProperty>

   <owl:ObjectProperty rdf:about="http://www.omg.org/spec/EDMC-SR/BE/OwnershipAndControl/ControlParties/basedOnInvestmentEquity">
      <skos:definition>Investment Based De Facto Control is based on the holding of some Investment Equity by some party.</skos:definition>
      <rdfs:subPropertyOf rdf:resource="http://www.omg.org/spec/EDMC-SR/FND/Relations/Relations/isConferredBy"/>
      <rdfs:domain rdf:resource="http://www.omg.org/spec/EDMC-SR/BE/OwnershipAndControl/ControlParties/InvestmentBasedDeFactoControl"/>
      <rdfs:range rdf:resource="http://www.omg.org/spec/EDMC-SR/BE/OwnershipAndControl/OwnershipParties/InvestmentEquity"/>
   </owl:ObjectProperty>

   <owl:ObjectProperty rdf:about="http://www.omg.org/spec/EDMC-SR/BE/OwnershipAndControl/ControlParties/isControlledToSomeDegreeBy">
      <skos:definition>Some party which has some degree of control over the organization.</skos:definition>
      <skos:editorialNote>Control by this type of party is either asserted to be the case by the entity itself or some other party, or is determined through some analysis or calculation based on the available information about controlling interests.</skos:editorialNote>
      <rdfs:subPropertyOf rdf:resource="http://www.omg.org/spec/EDMC-SR/FND/Relations/Relations/isControlledBy"/>
      <rdfs:domain rdf:resource="http://www.omg.org/spec/EDMC-SR/BE/LegalEntities/FormalBusinessOrganizations/FormallyConstitutedOrganization"/>
      <rdfs:range rdf:resource="http://www.omg.org/spec/EDMC-SR/BE/OwnershipAndControl/ControlParties/EntityControllingParty"/>
   </owl:ObjectProperty>

   <!--Data Properties-->

<owl:DatatypeProperty rdf:about="http://www.omg.org/spec/EDMC-SR/BE/OwnershipAndControl/ControlParties/percentageDeFactoControl">
      <rdfs:range rdf:resource="http://www.omg.org/spec/EDMC-SR/FND/Utilities/BusinessFacingTypes/percentage"/>
   </owl:DatatypeProperty>

   <owl:DatatypeProperty rdf:about="http://www.omg.org/spec/EDMC-SR/BE/OwnershipAndControl/ControlParties/percentageDeFactoControl.1">
      <rdfs:range rdf:resource="http://www.omg.org/spec/EDMC-SR/FND/Utilities/BusinessFacingTypes/percentage"/>
   </owl:DatatypeProperty>

   <!--Annotation Properties-->

<!--Classes-->

<owl:Class rdf:about="http://www.omg.org/spec/EDMC-SR/BE/OwnershipAndControl/ControlParties/COCOBondholder">
      <rdfs:label>COCO Bondholder</rdfs:label>
      <skos:definition>Holder of bank bonds which convert to equity holdings in a bank.</skos:definition>
      <skos:editorialNote>These equity holdings, when they exist, will confer upon the holder some de jure controlling interest in the issuing entity.</skos:editorialNote>
      <rdfs:subClassOf rdf:resource="http://www.omg.org/spec/EDMC-SR/BE/OwnershipAndControl/ControlParties/PartyHoldingSomeOptionForControl"/>
   </owl:Class>

   <owl:Class rdf:about="http://www.omg.org/spec/EDMC-SR/BE/OwnershipAndControl/ControlParties/ConstitutionalContractualControl">
      <rdfs:label>Constitutional Contractual Control</rdfs:label>
      <skos:definition>Some control set out in some contract among the principals of an organization.</skos:definition>
      <skos:editorialNote>This distinguishes this control from control conferred by contracts with third parties, for example in relation to third party guarantees or similar. This combines all forms of constitutional control in one set of terms under Constitutional De Jure Control.</skos:editorialNote>
      <rdfs:subClassOf rdf:resource="http://www.omg.org/spec/EDMC-SR/BE/OwnershipAndControl/ControlParties/ConstitutionalDeJureControl"/>
      <rdfs:subClassOf rdf:resource="http://www.omg.org/spec/EDMC-SR/BE/OwnershipAndControl/ControlParties/ContractualControl"/>
   </owl:Class>

   <owl:Class rdf:about="http://www.omg.org/spec/EDMC-SR/BE/OwnershipAndControl/ControlParties/ConstitutionalDeJureControl">
      <rdfs:label>Constitutional De Jure Control</rdfs:label>
      <skos:definition>Control which is based in some instrument which has constitutional standing (is constitutive of the entity) such as voting shares, general partner equity etc.</skos:definition>
      <rdfs:subClassOf rdf:resource="http://www.omg.org/spec/EDMC-SR/BE/OwnershipAndControl/ControlParties/DeJureControllingInterest"/>
   </owl:Class>

   <owl:Class rdf:about="http://www.omg.org/spec/EDMC-SR/BE/OwnershipAndControl/ControlParties/ContractualControl">
      <rdfs:label>Contractual  Control</rdfs:label>
      <skos:definition>Control vested in an entity by virtue of the terms in some contract between that entity and others.</skos:definition>
      <skos:editorialNote>See SME REview note of 16 Jan 2013: Percentage mechanism (in contracts etc.) would be factored in. Hence percentages as contractual terms. For instance an option to exercise which would give another 5% control. So there is % control with or without share ownership. Example: In a partnership this might be in the Partnership Agreement, which would identify beneficial ownership and control as potentially 2 distinct things. Contract can say anything. Implications: This means that there are percentages of de jure control based in contract, similar to those based in constitutional instruments (shares, General Partner equity). The concepts of Parent, Siinificant Part Owner etc. can then potentially be defined int erms of the percentages of all applicable instruments by which control may be formally defined.</skos:editorialNote>
      <rdfs:subClassOf rdf:resource="http://www.omg.org/spec/EDMC-SR/FND/OwnershipAndControl/Control/DeJureControl"/>
   </owl:Class>

   <owl:Class rdf:about="http://www.omg.org/spec/EDMC-SR/BE/OwnershipAndControl/ControlParties/ContractualControllingParty">
      <rdfs:label>Contractual Controlling Party</rdfs:label>
      <skos:definition>A party which exercises some control which is set out in some contract.</skos:definition>
      <skos:editorialNote>This is as distinct from control set out in some constitutional instrument e.g. voting shares ownership or general partner equity.</skos:editorialNote>
      <rdfs:subClassOf rdf:resource="http://www.omg.org/spec/EDMC-SR/BE/OwnershipAndControl/ControlParties/DeJureControllingInterestParty"/>
   </owl:Class>

   <owl:Class rdf:about="http://www.omg.org/spec/EDMC-SR/BE/OwnershipAndControl/ControlParties/ControlledParty">
      <rdfs:label>Controlled Party</rdfs:label>
      <skos:definition>Some party which is controlled in some way and to some degree by some other party.</skos:definition>
      <skos:editorialNote>Scope Note: Parties, since they stand in roles, will have relationships among them which correspond to the reciprocals of the roles they stand in. In this case, controls and controlled by.</skos:editorialNote>
      <rdfs:subClassOf rdf:resource="http://www.omg.org/spec/EDMC-SR/FND/Parties/Parties/PartyInRole"/>
   </owl:Class>

   <owl:Class rdf:about="http://www.omg.org/spec/EDMC-SR/BE/OwnershipAndControl/ControlParties/ControllingAlliance">
      <rdfs:label>Controlling Alliance</rdfs:label>
      <skos:definition>Some group of entities which have formed some alliance or agreement in terms of which they jointly exercise control over some entity.</skos:definition>
      <skos:editorialNote>The types of entity which may enter into such an alliance are the same types of entity as may exercise control in their own right, i.e. Involved Party (that is a logical union of natural persons, legal persons and formal organizations).</skos:editorialNote>
      <rdfs:subClassOf rdf:resource="http://www.omg.org/spec/EDMC-SR/FND/Organizations/FormalOrganizations/Group"/>
   </owl:Class>

   <owl:Class rdf:about="http://www.omg.org/spec/EDMC-SR/BE/OwnershipAndControl/ControlParties/ControllingInterestOptionHolder">
      <rdfs:label>Controlling Interest Option Holder</rdfs:label>
      <skos:definition>A party which holds some option which may be exercised to confer on that party some de jure controlling interest at some time in the future and at the discretion of that holder.</skos:definition>
   </owl:Class>

   <owl:Class rdf:about="http://www.omg.org/spec/EDMC-SR/BE/OwnershipAndControl/ControlParties/ControllingInterestParty">
      <rdfs:label>Controlling Interest Party</rdfs:label>
      <skos:definition>Some Party which holds some form of controlling interest in some other party in some context.</skos:definition>
      <skos:editorialNote>This controlling interest inevitably means that the party exercises some form of control, however the precise degree and nature of that control is dependent on many factors, and so is defined as a separate "Party" role (which may and usually is fulfilled by the same entity).</skos:editorialNote>
      <rdfs:subClassOf rdf:resource="http://www.omg.org/spec/EDMC-SR/FND/OwnershipAndControl/Control/ControllingParty"/>
   </owl:Class>

   <owl:Class rdf:about="http://www.omg.org/spec/EDMC-SR/BE/OwnershipAndControl/ControlParties/ControllingLeverageParty">
      <rdfs:label>Controlling Leverage Party</rdfs:label>
      <skos:definition>A party which exercises control as a result of some investment in an equity.</skos:definition>
      <skos:editorialNote>Any large investor may have some degree of de facto control.</skos:editorialNote>
      <rdfs:subClassOf rdf:resource="http://www.omg.org/spec/EDMC-SR/BE/OwnershipAndControl/ControlParties/DeFactoControllingInterestParty"/>
   </owl:Class>

   <owl:Class rdf:about="http://www.omg.org/spec/EDMC-SR/BE/OwnershipAndControl/ControlParties/CourtAppointedControl">
      <rdfs:label>Court Appointed Control</rdfs:label>
      <skos:definition>Control conferred on some entity by act of some court, for example in the context of receivership.</skos:definition>
   </owl:Class>

   <owl:Class rdf:about="http://www.omg.org/spec/EDMC-SR/BE/OwnershipAndControl/ControlParties/DeFactoControllingInterestParty">
      <rdfs:label>De Facto Controlling Interest Party</rdfs:label>
      <rdfs:subClassOf rdf:resource="http://www.omg.org/spec/EDMC-SR/BE/OwnershipAndControl/ControlParties/ControllingInterestParty"/>
   </owl:Class>

   <owl:Class rdf:about="http://www.omg.org/spec/EDMC-SR/BE/OwnershipAndControl/ControlParties/DeJureControllingInterest">
      <rdfs:label>De Jure Controlling Interest</rdfs:label>
      <skos:definition>Control which is formalized by some formal legal construct.</skos:definition>
   </owl:Class>

   <owl:Class rdf:about="http://www.omg.org/spec/EDMC-SR/BE/OwnershipAndControl/ControlParties/DeJureControllingInterestParty">
      <rdfs:label>De Jure Controlling Interest Party</rdfs:label>
      <skos:definition>An entity which exercises de jure control.</skos:definition>
   </owl:Class>

   <owl:Class rdf:about="http://www.omg.org/spec/EDMC-SR/BE/OwnershipAndControl/ControlParties/DegreeOfControl">
      <rdfs:label>Degree Of Control</rdfs:label>
   </owl:Class>

   <owl:Class rdf:about="http://www.omg.org/spec/EDMC-SR/BE/OwnershipAndControl/ControlParties/EntityControllingParty">
      <rdfs:label>Entity Controlling Party</rdfs:label>
      <skos:definition>Some party which is able to direct the activities of some business entity.</skos:definition>
      <skos:editorialNote>This type of party is either asserted to be the case by the entity itself or some other party, or is determined through some analysis or calculation based on the available information about controlling interests.</skos:editorialNote>
   </owl:Class>

   <owl:Class rdf:about="http://www.omg.org/spec/EDMC-SR/BE/OwnershipAndControl/ControlParties/EquityBasedDeJureControl">
      <rdfs:label>Equity Based De Jure Control</rdfs:label>
      <skos:definition>De Jure controlling interest in an entity which is based on the holding of some form of equity in that entity.</skos:definition>
   </owl:Class>

   <owl:Class rdf:about="http://www.omg.org/spec/EDMC-SR/BE/OwnershipAndControl/ControlParties/InfluenceBasedDeFactoControl">
      <rdfs:label>Influence Based De Facto Control</rdfs:label>
      <skos:definition>Some influence and control over some entity other than by means of investment in that entity.</skos:definition>
      <rdfs:subClassOf rdf:resource="http://www.omg.org/spec/EDMC-SR/FND/OwnershipAndControl/Control/DeFactoControl"/>
   </owl:Class>

   <owl:Class rdf:about="http://www.omg.org/spec/EDMC-SR/BE/OwnershipAndControl/ControlParties/InfluenceBasedDeFactoControllingParty">
      <rdfs:label>Influence Based De Facto Controlling Party</rdfs:label>
      <skos:definition>A party which exercises some influence and control over the entity other than by means of investment.</skos:definition>
      <skos:editorialNote>Regulatory or jurisdictional control would fall under this control. Court appointed control is de jure control BUT the scenario in which a government takes over something and then hands it over to some new de jure controller i.e. administrator - in the meantime this is de facto control by e.g. the government.</skos:editorialNote>
   </owl:Class>

   <owl:Class rdf:about="http://www.omg.org/spec/EDMC-SR/BE/OwnershipAndControl/ControlParties/InvestmentBasedDeFactoControl">
      <rdfs:label>Investment Based De Facto Control</rdfs:label>
      <skos:definition>Control which arises through some investment in some entity, other than as the holding of "constitutional" equity (shares etc.) in that entity.</skos:definition>
   </owl:Class>

   <owl:Class rdf:about="http://www.omg.org/spec/EDMC-SR/BE/OwnershipAndControl/ControlParties/InvestmentBasedDeFactoControllingInterestParty">
      <rdfs:label>Investment Based De Facto Controlling Interest Party</rdfs:label>
      <skos:definition>A party which exercises some degree of de facto control based on some investment which they hold in the entity.</skos:definition>
      <rdfs:subClassOf rdf:resource="http://www.omg.org/spec/EDMC-SR/BE/OwnershipAndControl/OwnershipParties/Investor"/>
   </owl:Class>

   <owl:Class rdf:about="http://www.omg.org/spec/EDMC-SR/BE/OwnershipAndControl/ControlParties/JointControllingParty">
      <rdfs:label>Joint Controlling Party</rdfs:label>
      <rdfs:subClassOf rdf:resource="http://www.omg.org/spec/EDMC-SR/BE/OwnershipAndControl/ControlParties/EntityControllingParty"/>
   </owl:Class>

   <owl:Class rdf:about="http://www.omg.org/spec/EDMC-SR/BE/OwnershipAndControl/ControlParties/LimitedControllingParty">
      <rdfs:label>Limited Controlling Party</rdfs:label>
      <skos:definition>Some individual entity which is able to direct the affairs of some business organization to a specific degree.</skos:definition>
      <skos:editorialNote>The degree to which the party has control of (is able to direct the activities of) the organization in question is defined as a percentage value where one hundred percent would equate to control without the involvement of others. The percentage of control is a calculated, determined or asserted value, and not necessarily a percentage of some controlling interest, though in the absence of other factors the determination of percentage of control would equate to the percentage of controlling interest e.g. voting shares held.</skos:editorialNote>
   </owl:Class>

   <owl:Class rdf:about="http://www.omg.org/spec/EDMC-SR/BE/OwnershipAndControl/ControlParties/LimitedDeFactoControl">
      <rdfs:label>Limited De Facto Control</rdfs:label>
      <skos:definition>The ability to direct the affairs of some entity within prescribed limits. Those limits are described in terms of activities which the entity holding such control may cause the controlled entity to carry out.</skos:definition>
   </owl:Class>

   <owl:Class rdf:about="http://www.omg.org/spec/EDMC-SR/BE/OwnershipAndControl/ControlParties/MajorityControllingParty">
      <rdfs:label>Majority Controlling Party</rdfs:label>
      <rdfs:subClassOf rdf:resource="http://www.omg.org/spec/EDMC-SR/BE/OwnershipAndControl/ControlParties/SoleControllingParty"/>
   </owl:Class>

   <owl:Class rdf:about="http://www.omg.org/spec/EDMC-SR/BE/OwnershipAndControl/ControlParties/PartyHoldingSomeOptionForControl">
      <rdfs:label>Party Holding Some Option for Control</rdfs:label>
      <skos:definition>Some party holding the option to exercise some De Jure Controlling Interest</skos:definition>
      <skos:editorialNote>This will result in some potential change at a future time, in the conclusions about actual control.</skos:editorialNote>
   </owl:Class>

   <owl:Class rdf:about="http://www.omg.org/spec/EDMC-SR/BE/OwnershipAndControl/ControlParties/Receiver">
      <rdfs:label>Receiver</rdfs:label>
      <skos:definition>A party appointed by some court for the purposes of winding up the affais of some entity which is no longer solvent.</skos:definition>
   </owl:Class>

   <owl:Class rdf:about="http://www.omg.org/spec/EDMC-SR/BE/OwnershipAndControl/ControlParties/SignificantControllingInterestParty">
      <rdfs:label>Significant Controlling Interest Party</rdfs:label>
      <skos:definition>A person which owns a significant voting stake in this entity of between some lower significant threshold and 50%, but not 50% or more.</skos:definition>
   </owl:Class>

   <owl:Class rdf:about="http://www.omg.org/spec/EDMC-SR/BE/OwnershipAndControl/ControlParties/SoleControllingParty">
      <rdfs:label>Sole Controlling Party</rdfs:label>
      <skos:definition>Some individual entity which is able to direct the affairs of some business organization to some degree.</skos:definition>
   </owl:Class>

   <owl:Class rdf:about="http://www.omg.org/spec/EDMC-SR/BE/OwnershipAndControl/ControlParties/TotalOwner">
      <rdfs:label>Total Owner</rdfs:label>
      <skos:definition>Entity having 100% ownership in the entity so owned.</skos:definition>
      <skos:editorialNote>By virtue of holding 100% of the equity ownership, the Total Owner also holds 100% of the controlling equity, if there is a difference. Therefore it is both a total owner and a total controlling party.</skos:editorialNote>
      <rdfs:subClassOf rdf:resource="http://www.omg.org/spec/EDMC-SR/BE/OwnershipAndControl/OwnershipParties/ConstitutionalOwner"/>
   </owl:Class>

   <owl:Class rdf:about="http://www.omg.org/spec/EDMC-SR/BE/OwnershipAndControl/ControlParties/WarrantHolder">
      <rdfs:label>Warrant Holder</rdfs:label>
      <skos:definition>A holder of some warrant which when exercised would confer upon that party some de jure controlling interest in some entity.</skos:definition>
   </owl:Class>

   <!--Individuals-->

<owl:NamedIndividual rdf:about="http://www.omg.org/spec/EDMC-SR/BE/OwnershipAndControl/ControlParties/http...www.ecfr.gov.cgi-bin.retrieveECFR?gp=1&amp;SID=156b3a57ae63855b0de1b32e322c998a&amp;ty=HTML&amp;h=L&amp;r=PART&amp;n=17y2.0.1.1.8#17.2.0.1.1.8.0.17.2">
      <rdf:Type rdf:resource="http://www.edmcouncil.org/spec/EDMC-SR/FND/Publications/Publications/WebPage"/>
   </owl:NamedIndividual>

</rdf:RDF>