<?xml version="1.0" encoding="UTF-8"?>
<rdf:RDF xmlns:xsd="http://www.w3.org/2001/XMLSchema#"
         xmlns:sm="http://www.omg.org/techprocess/ab/SpecificationMetadata/"
         xmlns:fibo-fnd-utl-av="http://www.omg.org/spec/EDMC-FIBO/FND/Utilities/AnnotationVocabulary/"
         xmlns:rdf="http://www.w3.org/1999/02/22-rdf-syntax-ns#"
         xmlns:rdfs="http://www.w3.org/2000/01/rdf-schema#"
         xmlns:owl="http://www.w3.org/2002/07/owl#"
         xmlns:skos="http://www.w3.org/2004/02/skos/core#"
         xmlns:dc="http://purl.org/dc/terms/"
         xml:base="http://www.omg.org/spec/EDMC-SR/BE/OwnershipAndControl/CorporateOwnership/">

   <owl:Ontology rdf:about="http://www.omg.org/spec/EDMC-SR/BE/OwnershipAndControl/CorporateOwnership/">
      <owl:imports rdf:resource="http://www.omg.org/spec/EDMC-FIBO/SEC/Securities/SecurityAssets/"/>
      <owl:imports rdf:resource="http://www.omg.org/spec/EDMC-SR/BE/OwnershipAndControl/OwnershipParties/"/>
      <owl:imports rdf:resource="http://www.omg.org/spec/EDMC-SR/BE/Corporations/Corporations/"/>
      <owl:imports rdf:resource="http://www.omg.org/spec/EDMC-FIBO/SEC/Equities/EquityInstruments/"/>
   </owl:Ontology>

   <!--Datatypes-->

<!--Object Properties-->

<owl:ObjectProperty rdf:about="http://www.omg.org/spec/EDMC-SR/BE/OwnershipAndControl/CorporateOwnership/shareholderHoldsAnInterestIn">
      <skos:definition>The Shareholder owns some stake in the Incorporated company for example by virtue of owning some shares.</skos:definition>
      <rdfs:subPropertyOf rdf:resource="http://www.omg.org/spec/EDMC-SR/BE/OwnershipAndControl/OwnershipParties/holdsAnInterestIn"/>
      <rdfs:domain rdf:resource="http://www.omg.org/spec/EDMC-SR/BE/OwnershipAndControl/CorporateOwnership/Shareholder"/>
      <rdfs:range rdf:resource="http://www.omg.org/spec/EDMC-SR/BE/Corporations/Corporations/IncorporatedCompany"/>
   </owl:ObjectProperty>

   <owl:ObjectProperty rdf:about="http://www.omg.org/spec/EDMC-SR/BE/OwnershipAndControl/CorporateOwnership/shareholderHoldsEquity">
      <skos:definition>The shareholder holds some of the issued shareholder equity in the company, by way of the shares that they hold. This is a kind of Stockholders Equity.</skos:definition>
      <rdfs:subPropertyOf rdf:resource="http://www.omg.org/spec/EDMC-SR/BE/OwnershipAndControl/OwnershipParties/holdsSomeStockholderEquity"/>
      <rdfs:domain rdf:resource="http://www.omg.org/spec/EDMC-SR/BE/OwnershipAndControl/CorporateOwnership/Shareholder"/>
      <rdfs:range rdf:resource="http://www.omg.org/spec/EDMC-SR/FND/Accounting/AccountingEquity/StockholdersEquity"/>
   </owl:ObjectProperty>

   <owl:ObjectProperty rdf:about="http://www.omg.org/spec/EDMC-SR/BE/OwnershipAndControl/CorporateOwnership/heldBy">
      <skos:definition>The holder of the shares, that is the party of which this is the shareholding.</skos:definition>
      <rdfs:subPropertyOf rdf:resource="http://www.omg.org/spec/EDMC-FIBO/SEC/Securities/SecurityAssets/heldBy"/>
      <rdfs:subPropertyOf rdf:resource="http://www.omg.org/spec/EDMC-SR/FND/OwnershipAndControl/Ownership/isAssetOf"/>
      <rdfs:domain rdf:resource="http://www.omg.org/spec/EDMC-SR/BE/OwnershipAndControl/CorporateOwnership/Shareholding"/>
      <rdfs:range rdf:resource="http://www.omg.org/spec/EDMC-SR/BE/OwnershipAndControl/CorporateOwnership/Shareholder"/>
   </owl:ObjectProperty>

   <!--Data Properties-->

<!--Annotation Properties-->

<!--Classes-->

<owl:Class rdf:about="http://www.omg.org/spec/EDMC-SR/BE/OwnershipAndControl/CorporateOwnership/BeneficialOwner">
      <rdfs:label>Beneficial Owner</rdfs:label>
      <skos:definition>Some entity which owns some stake in the company (voting or non voting) and exercises some control either through that ownership or by some other means.</skos:definition>
      <skos:editorialNote>This covers entities which have any kind of control. From World Bank Report: "In identifying the beneficial owner, the focus should be on two factors: the control exercised and the benefit derived. Control of a corporate vehicle will always depend on context, as control can be exercised in many different ways, including through ownership, contractually or informally."</skos:editorialNote>
      <rdfs:subClassOf rdf:resource="http://www.omg.org/spec/EDMC-SR/BE/OwnershipAndControl/CorporateOwnership/Shareholder"/>
   </owl:Class>

   <owl:Class rdf:about="http://www.omg.org/spec/EDMC-SR/BE/OwnershipAndControl/CorporateOwnership/PublicShareholder">
      <rdfs:label>Public Shareholder</rdfs:label>
      <skos:definition>A party that holds publicly issued shares in a listed company.</skos:definition>
   </owl:Class>

   <owl:Class rdf:about="http://www.omg.org/spec/EDMC-SR/BE/OwnershipAndControl/CorporateOwnership/RegisteredShareholder">
      <rdfs:label>Registered Shareholder</rdfs:label>
      <skos:definition>A shareholder which is registered as such on the company shareholder register for that company.</skos:definition>
   </owl:Class>

   <owl:Class rdf:about="http://www.omg.org/spec/EDMC-SR/BE/OwnershipAndControl/CorporateOwnership/Shareholder">
      <rdfs:label>Shareholder</rdfs:label>
      <skos:definition>A party owning shares in some company limited by the issue of shares.</skos:definition>
      <rdfs:subClassOf rdf:resource="http://www.omg.org/spec/EDMC-SR/FND/Agreements/Contracts/TransferableContractHolder"/>
      <rdfs:subClassOf rdf:resource="http://www.omg.org/spec/EDMC-SR/BE/OwnershipAndControl/OwnershipParties/ConstitutionalOwner"/>
      <rdfs:subClassOf rdf:resource="http://www.omg.org/spec/EDMC-FIBO/SEC/Securities/SecurityAssets/SecurityHolder"/>
   </owl:Class>

   <owl:Class rdf:about="http://www.omg.org/spec/EDMC-SR/BE/OwnershipAndControl/CorporateOwnership/Shareholding">
      <rdfs:label>Shareholding</rdfs:label>
      <skos:definition>The holding of some Share.</skos:definition>
      <rdfs:subClassOf rdf:resource="http://www.omg.org/spec/EDMC-SR/FND/OwnershipAndControl/Ownership/Asset"/>
      <rdfs:subClassOf rdf:resource="http://www.omg.org/spec/EDMC-FIBO/SEC/Securities/SecurityAssets/SecurityHolding"/>
   </owl:Class>

   <!--Individuals-->

</rdf:RDF>