<?xml version="1.0" encoding="UTF-8"?>
<rdf:RDF xmlns:xsd="http://www.w3.org/2001/XMLSchema#"
         xmlns:sm="http://www.omg.org/techprocess/ab/SpecificationMetadata/"
         xmlns:fibo-fnd-utl-av="http://www.omg.org/spec/EDMC-FIBO/FND/Utilities/AnnotationVocabulary/"
         xmlns:rdf="http://www.w3.org/1999/02/22-rdf-syntax-ns#"
         xmlns:rdfs="http://www.w3.org/2000/01/rdf-schema#"
         xmlns:owl="http://www.w3.org/2002/07/owl#"
         xmlns:skos="http://www.w3.org/2004/02/skos/core#"
         xmlns:dc="http://purl.org/dc/terms/"
         xml:base="http://www.omg.org/spec/EDMC-SR/BE/OwnershipAndControl/CorporateControl/">

   <owl:Ontology rdf:about="http://www.omg.org/spec/EDMC-SR/BE/OwnershipAndControl/CorporateControl/">
      <owl:imports rdf:resource="http://www.omg.org/spec/EDMC-SR/BE/OwnershipAndControl/CorporateOwnership/"/>
      <owl:imports rdf:resource="http://www.omg.org/spec/EDMC-SR/BE/OwnershipAndControl/ControlParties/"/>
   </owl:Ontology>

   <!--Datatypes-->

<!--Object Properties-->

<owl:ObjectProperty rdf:about="http://www.omg.org/spec/EDMC-SR/BE/OwnershipAndControl/CorporateControl/controlledCompanyIdentity">
      <skos:definition>That Formal Organization which is identified as a controlled company.</skos:definition>
      <skos:editorialNote>This forms the basis for an entity being defined as a Subsidiary.</skos:editorialNote>
      <rdfs:subPropertyOf rdf:resource="http://www.omg.org/spec/EDMC-SR/FND/Parties/Parties/partyInRoleHasIdentity"/>
      <rdfs:domain rdf:resource="http://www.omg.org/spec/EDMC-SR/BE/OwnershipAndControl/CorporateControl/ControlledCompany"/>
      <rdfs:range rdf:resource="http://www.omg.org/spec/EDMC-SR/BE/LegalEntities/FormalBusinessOrganizations/FormallyConstitutedOrganization"/>
   </owl:ObjectProperty>

   <owl:ObjectProperty rdf:about="http://www.omg.org/spec/EDMC-SR/BE/OwnershipAndControl/CorporateControl/incorporatedCompanyHasControllingInterestParty">
      <skos:definition>Some control of the Incorporated Company is wielded by some Voting Shareholder.</skos:definition>
      <skos:editorialNote>This control is by means of voting equity in the form of voting shares, which gives the shareholder a say in the running of the company.</skos:editorialNote>
      <rdfs:subPropertyOf rdf:resource="http://www.omg.org/spec/EDMC-SR/BE/OwnershipAndControl/ControlParties/hasControllingInterestParty"/>
      <rdfs:domain rdf:resource="http://www.omg.org/spec/EDMC-SR/BE/Corporations/Corporations/IncorporatedCompany"/>
      <rdfs:range rdf:resource="http://www.omg.org/spec/EDMC-SR/BE/OwnershipAndControl/CorporateControl/VotingShareholder"/>
   </owl:ObjectProperty>

   <owl:ObjectProperty rdf:about="http://www.omg.org/spec/EDMC-SR/BE/OwnershipAndControl/CorporateControl/incprporatedCompanyHasSignificantControllingInterestCompany">
      <rdfs:subPropertyOf rdf:resource="http://www.omg.org/spec/EDMC-SR/BE/OwnershipAndControl/ControlParties/hasSignificantControllingInterstParty"/>
      <rdfs:domain rdf:resource="http://www.omg.org/spec/EDMC-SR/BE/Corporations/Corporations/IncorporatedCompany"/>
      <rdfs:range rdf:resource="http://www.omg.org/spec/EDMC-SR/BE/OwnershipAndControl/CorporateControl/SignificantShareholdingCompany"/>
      <owl:inverseOf rdf:resource="http://www.omg.org/spec/EDMC-SR/BE/OwnershipAndControl/CorporateControl/holdsSignificantControllingInterestIn"/>
   </owl:ObjectProperty>

   <owl:ObjectProperty rdf:about="http://www.omg.org/spec/EDMC-SR/BE/OwnershipAndControl/CorporateControl/hasVotingRights">
      <skos:definition>The Voting Shareholder holds certain Voting Rights as a consequence of their holding of those shares.</skos:definition>
      <rdfs:subPropertyOf rdf:resource="http://www.omg.org/spec/EDMC-SR/BE/OwnershipAndControl/CorporateControl/holdsSome"/>
      <rdfs:domain rdf:resource="http://www.omg.org/spec/EDMC-SR/BE/OwnershipAndControl/CorporateControl/VotingShareholder"/>
      <rdfs:range rdf:resource="http://www.omg.org/spec/EDMC-FIBO/SEC/Equities/EquityInstruments/VotingRight"/>
   </owl:ObjectProperty>

   <owl:ObjectProperty rdf:about="http://www.omg.org/spec/EDMC-SR/BE/OwnershipAndControl/CorporateControl/holdsSome">
      <skos:definition>Voting Shareholder is the holder of some Voting Share.</skos:definition>
      <rdfs:domain rdf:resource="http://www.omg.org/spec/EDMC-SR/BE/OwnershipAndControl/CorporateControl/VotingShareholder"/>
      <rdfs:range rdf:resource="http://www.omg.org/spec/EDMC-FIBO/SEC/Equities/EquityInstruments/VotingShare"/>
   </owl:ObjectProperty>

   <owl:ObjectProperty rdf:about="http://www.omg.org/spec/EDMC-SR/BE/OwnershipAndControl/CorporateControl/votingShareholdingCompanyHasIdentity">
      <skos:definition>The Shareholding Company is a Formal Organization.</skos:definition>
      <skos:editorialNote>This may be any Body Corporate, including other Incorporated Companies, but also may be a Trust or other non incorporated Formal Organization. Scope Note: This is the defining fact about the party which is a Shareholding Company. All the types of party which are derived from this, are defined as not only being shareholders, but also being themselves Formal Organizations.</skos:editorialNote>
      <rdfs:subPropertyOf rdf:resource="http://www.edmcouncil.org/spec/EDMC-SR/BE/OwnershipAndControlExt/OwnershipPartiesExtras/entityOwningPartyIdentity"/>
      <rdfs:subPropertyOf rdf:resource="http://www.omg.org/spec/EDMC-SR/FND/Parties/Parties/partyInRoleHasIdentity"/>
      <rdfs:domain rdf:resource="http://www.omg.org/spec/EDMC-SR/BE/OwnershipAndControl/CorporateControl/VotingShareholdingCompany"/>
      <rdfs:range rdf:resource="http://www.omg.org/spec/EDMC-SR/BE/LegalEntities/FormalBusinessOrganizations/FormallyConstitutedOrganization"/>
   </owl:ObjectProperty>

   <owl:ObjectProperty rdf:about="http://www.omg.org/spec/EDMC-SR/BE/OwnershipAndControl/CorporateControl/votingShareholdingCompanyHoldsControllingInterestIn">
      <skos:definition>A registered company which is a part or subsidiary of the Incorporated Company in the same or another Jurisdiction.</skos:definition>
      <rdfs:subPropertyOf rdf:resource="http://www.omg.org/spec/EDMC-SR/BE/OwnershipAndControl/CorporateControl/holdsControllingInterestIn"/>
      <rdfs:domain rdf:resource="http://www.omg.org/spec/EDMC-SR/BE/OwnershipAndControl/CorporateControl/VotingShareholdingCompany"/>
      <rdfs:range rdf:resource="http://www.omg.org/spec/EDMC-SR/BE/Corporations/Corporations/IncorporatedCompany"/>
   </owl:ObjectProperty>

   <owl:ObjectProperty rdf:about="http://www.omg.org/spec/EDMC-SR/BE/OwnershipAndControl/CorporateControl/heldBy">
      <skos:definition>The holder of the Voting Shares, that is the party of which this is the shareholding and which therefore enjoys the voting rights thereof.</skos:definition>
      <rdfs:subPropertyOf rdf:resource="http://www.omg.org/spec/EDMC-SR/BE/OwnershipAndControl/CorporateOwnership/heldBy"/>
      <rdfs:domain rdf:resource="http://www.omg.org/spec/EDMC-SR/BE/OwnershipAndControl/CorporateControl/VotingShareholding"/>
      <rdfs:range rdf:resource="http://www.omg.org/spec/EDMC-SR/BE/OwnershipAndControl/CorporateControl/VotingShareholder"/>
   </owl:ObjectProperty>

   <owl:ObjectProperty rdf:about="http://www.omg.org/spec/EDMC-SR/BE/OwnershipAndControl/CorporateControl/hasAffiliarte">
      <skos:definition>Ownership between some minimum percentage and majority holding. That minimum percentage is determined in local law and may be for example 10% or 25%.</skos:definition>
      <skos:editorialNote>Affiliated company: Associated or affiliated with (synonyms). Definition from BusinessDirectory.com for Associate: Firm over which another firm exercises a degree of control which is less than the degree of control exercised over a subsidiary. In accounting, such control is typically taken to mean the ownership of at least 20 percent of voting shares, and some say in the management of the associate firm. Associated companies usually have interlocking directorates to ensure they have common policies and complementary objectives. Additional Notes: Uni of Melbourne: Associate in corporations Law: one of the most important definitions in the corp law is associate. Regulate takeovers compulsory acquisitions and other transactions. Now 2 definitions which are not entirely consistent (one does not repeal the other). Associate is a person in this sense. Definition origin: businessdictionary.com</skos:editorialNote>
      <rdfs:subPropertyOf rdf:resource="http://www.omg.org/spec/EDMC-SR/BE/OwnershipAndControl/ControlParties/hasControllingInterestParty"/>
      <rdfs:domain rdf:resource="http://www.omg.org/spec/EDMC-SR/BE/Corporations/Corporations/IncorporatedCompany"/>
      <rdfs:range rdf:resource="http://www.omg.org/spec/EDMC-SR/BE/OwnershipAndControl/CorporateControl/Affiliate"/>
   </owl:ObjectProperty>

   <owl:ObjectProperty rdf:about="http://www.omg.org/spec/EDMC-SR/BE/OwnershipAndControl/CorporateControl/hasControllingInterestPartyVotingShareholdingCompany">
      <rdfs:subPropertyOf rdf:resource="http://www.omg.org/spec/EDMC-SR/BE/OwnershipAndControl/CorporateControl/incorporatedCompanyHasControllingInterestParty"/>
      <rdfs:domain rdf:resource="http://www.omg.org/spec/EDMC-SR/BE/Corporations/Corporations/IncorporatedCompany"/>
      <rdfs:range rdf:resource="http://www.omg.org/spec/EDMC-SR/BE/OwnershipAndControl/CorporateControl/VotingShareholdingCompany"/>
      <owl:inverseOf rdf:resource="http://www.omg.org/spec/EDMC-SR/BE/OwnershipAndControl/CorporateControl/votingShareholdingCompanyHoldsControllingInterestIn"/>
   </owl:ObjectProperty>

   <owl:ObjectProperty rdf:about="http://www.omg.org/spec/EDMC-SR/BE/OwnershipAndControl/CorporateControl/hasDomesticUltimateParent">
      <skos:definition>The organization which is recognized as the ultimate parent of the company within the country or jurisdiction of incorporation. This relationship may or may not be present, i.e. in the case of a company which has no parent.</skos:definition>
      <skos:editorialNote>In the case of companies which are a subsidiary of another company which itself has a parent, this is the organization which sits at the top of the hierarchy of organizations in the country of registration of the company of which this is a property. Adapted from consensus definition of Ultimate Parent, now that this is split into national and global parent.</skos:editorialNote>
      <rdfs:subPropertyOf rdf:resource="http://www.omg.org/spec/EDMC-SR/BE/OwnershipAndControl/ControlParties/hasMajorityControllingParty"/>
      <rdfs:domain rdf:resource="http://www.omg.org/spec/EDMC-SR/BE/Corporations/Corporations/IncorporatedCompany"/>
      <rdfs:range rdf:resource="http://www.omg.org/spec/EDMC-SR/BE/OwnershipAndControl/CorporateControl/DomesticUltimateParent"/>
   </owl:ObjectProperty>

   <owl:ObjectProperty rdf:about="http://www.omg.org/spec/EDMC-SR/BE/OwnershipAndControl/CorporateControl/hasGlobalUltimateParent">
      <skos:definition>The organization which is recognized as the ultimate parent of the company. This relationship may or may not be present, i.e. in the case of a company which has no parent.</skos:definition>
      <skos:editorialNote>In the case of companies which are a subsidiary of another company which itself has a parent, this is the organization which sits at the top of the hierarchy of organizations worldwide.</skos:editorialNote>
      <rdfs:subPropertyOf rdf:resource="http://www.omg.org/spec/EDMC-SR/BE/OwnershipAndControl/ControlParties/hasMajorityControllingParty"/>
      <rdfs:domain rdf:resource="http://www.omg.org/spec/EDMC-SR/BE/Corporations/Corporations/IncorporatedCompany"/>
      <rdfs:range rdf:resource="http://www.omg.org/spec/EDMC-SR/BE/OwnershipAndControl/CorporateControl/GlobalUltimateParent"/>
   </owl:ObjectProperty>

   <owl:ObjectProperty rdf:about="http://www.omg.org/spec/EDMC-SR/BE/OwnershipAndControl/CorporateControl/hasMajorityControllingInterestParty">
      <skos:definition>The parent organization of the company, if there is one.</skos:definition>
      <skos:editorialNote>This is defined as company or other Formal Organization which owns a controlling stake of &amp;gt;50% (50% plus one voting share or above) in this company.</skos:editorialNote>
      <rdfs:subPropertyOf rdf:resource="http://www.omg.org/spec/EDMC-SR/BE/OwnershipAndControl/ControlParties/hasSignificantControllingInterstParty"/>
      <rdfs:domain rdf:resource="http://www.omg.org/spec/EDMC-SR/BE/Corporations/Corporations/IncorporatedCompany"/>
      <rdfs:range rdf:resource="http://www.omg.org/spec/EDMC-SR/BE/OwnershipAndControl/CorporateControl/OverFiftyPercentControlingInterestCompany"/>
   </owl:ObjectProperty>

   <owl:ObjectProperty rdf:about="http://www.omg.org/spec/EDMC-SR/BE/OwnershipAndControl/CorporateControl/hasMajorityOwnedSubsidiary">
      <skos:definition>A company which is recognized as a majority owned subsidiary of this company. This is where there is above 50% (50% plus one share) ownership of the shares.</skos:definition>
      <rdfs:subPropertyOf rdf:resource="http://www.omg.org/spec/EDMC-SR/BE/OwnershipAndControl/CorporateControl/hasSubsidiary"/>
      <rdfs:domain rdf:resource="http://www.omg.org/spec/EDMC-SR/BE/Corporations/Corporations/IncorporatedCompany"/>
      <rdfs:range rdf:resource="http://www.omg.org/spec/EDMC-SR/BE/OwnershipAndControl/CorporateControl/WhollyOwnedSubsidiary"/>
   </owl:ObjectProperty>

   <owl:ObjectProperty rdf:about="http://www.omg.org/spec/EDMC-SR/BE/OwnershipAndControl/CorporateControl/hasSubsidiary">
      <skos:definition>The company has control over some company, which is identified as a Subsidiary by virtue of this.</skos:definition>
      <rdfs:domain rdf:resource="http://www.omg.org/spec/EDMC-SR/BE/Corporations/Corporations/IncorporatedCompany"/>
      <rdfs:range rdf:resource="http://www.omg.org/spec/EDMC-SR/BE/OwnershipAndControl/CorporateControl/Subsidiary"/>
   </owl:ObjectProperty>

   <owl:ObjectProperty rdf:about="http://www.omg.org/spec/EDMC-SR/BE/OwnershipAndControl/CorporateControl/holdsControllingInterestIn">
      <skos:definition>The shareholder holds some voting stake in the Incorporated Company, by means of their holding of voting shares.</skos:definition>
      <rdfs:subPropertyOf rdf:resource="http://www.omg.org/spec/EDMC-SR/BE/OwnershipAndControl/OwnershipParties/holdsAnInterestIn"/>
      <rdfs:domain rdf:resource="http://www.omg.org/spec/EDMC-SR/BE/OwnershipAndControl/CorporateControl/VotingShareholder"/>
      <rdfs:range rdf:resource="http://www.omg.org/spec/EDMC-SR/BE/Corporations/Corporations/IncorporatedCompany"/>
   </owl:ObjectProperty>

   <owl:ObjectProperty rdf:about="http://www.omg.org/spec/EDMC-SR/BE/OwnershipAndControl/CorporateControl/holdsMajorityControllingInterestIn">
      <skos:definition>The Incorporated Company in which the party holds fifty percent or more of the voting share equity.</skos:definition>
      <rdfs:subPropertyOf rdf:resource="http://www.omg.org/spec/EDMC-SR/BE/OwnershipAndControl/CorporateControl/holdsControllingInterestIn"/>
      <rdfs:domain rdf:resource="http://www.omg.org/spec/EDMC-SR/BE/OwnershipAndControl/CorporateControl/VotingShareholder"/>
      <rdfs:range rdf:resource="http://www.omg.org/spec/EDMC-SR/BE/Corporations/Corporations/IncorporatedCompany"/>
   </owl:ObjectProperty>

   <owl:ObjectProperty rdf:about="http://www.omg.org/spec/EDMC-SR/BE/OwnershipAndControl/CorporateControl/holdsSignificantControllingInterestIn">
      <skos:definition>The Incorporated Company in which the party holds a significant proportion (but not fifty percent or more) of the voting share equity.</skos:definition>
      <rdfs:subPropertyOf rdf:resource="http://www.omg.org/spec/EDMC-SR/BE/OwnershipAndControl/CorporateControl/holdsControllingInterestIn"/>
      <rdfs:domain rdf:resource="http://www.omg.org/spec/EDMC-SR/BE/OwnershipAndControl/CorporateControl/VotingShareholder"/>
      <rdfs:range rdf:resource="http://www.omg.org/spec/EDMC-SR/BE/Corporations/Corporations/IncorporatedCompany"/>
   </owl:ObjectProperty>

   <owl:ObjectProperty rdf:about="http://www.omg.org/spec/EDMC-SR/BE/OwnershipAndControl/CorporateControl/exercisesEquityBasedDeJureControl">
      <skos:definition>A Voting Shareholder exercise some Equity Based de jure control in the entity for which they hold those shares.</skos:definition>
      <rdfs:subPropertyOf rdf:resource="http://www.omg.org/spec/EDMC-SR/BE/OwnershipAndControl/ControlParties/holdsSomeInstrumentOfDeJureControl"/>
      <rdfs:domain rdf:resource="http://www.omg.org/spec/EDMC-SR/BE/OwnershipAndControl/CorporateControl/VotingShareholder"/>
      <rdfs:range rdf:resource="http://www.omg.org/spec/EDMC-SR/BE/OwnershipAndControl/ControlParties/EquityBasedDeJureControl"/>
   </owl:ObjectProperty>

   <owl:ObjectProperty rdf:about="http://www.omg.org/spec/EDMC-SR/BE/OwnershipAndControl/CorporateControl/isWhollyOwnedBy">
      <skos:definition>The Incorporated Company is totally owned and therefore wholly controlled by some Formal Organization having 100% ownership in it.</skos:definition>
      <rdfs:subPropertyOf rdf:resource="http://www.omg.org/spec/EDMC-SR/BE/OwnershipAndControl/ControlParties/hasTotalOwner"/>
      <rdfs:subPropertyOf rdf:resource="http://www.omg.org/spec/EDMC-SR/BE/OwnershipAndControl/CorporateControl/hasMajorityControllingInterestParty"/>
      <rdfs:domain rdf:resource="http://www.omg.org/spec/EDMC-SR/BE/Corporations/Corporations/IncorporatedCompany"/>
      <rdfs:range rdf:resource="http://www.omg.org/spec/EDMC-SR/BE/OwnershipAndControl/CorporateControl/TotalControllingInterestCompany"/>
   </owl:ObjectProperty>

   <!--Data Properties-->

<!--Annotation Properties-->

<!--Classes-->

<owl:Class rdf:about="http://www.omg.org/spec/EDMC-SR/BE/OwnershipAndControl/CorporateControl/Anon-18737">
      <owl:equivalentClass>
         <owl:Class>
            <owl:unionOf rdf:parseType="Collection">
               <owl:Class rdf:about="http://www.omg.org/spec/EDMC-SR/FND/OwnershipAndControl/Control/ControllingParty"/>
               <owl:Class rdf:about="http://www.omg.org/spec/EDMC-SR/BE/OwnershipAndControl/CorporateControl/ControlledCompany"/>
            </owl:unionOf>
         </owl:Class>
      </owl:equivalentClass>
   </owl:Class>

   <owl:Class rdf:about="http://www.omg.org/spec/EDMC-SR/BE/OwnershipAndControl/CorporateControl/Affiliate">
      <rdfs:label>Affiliate</rdfs:label>
   </owl:Class>

   <owl:Class rdf:about="http://www.omg.org/spec/EDMC-SR/BE/OwnershipAndControl/CorporateControl/ControlledCompany">
      <rdfs:label>Controlled Company</rdfs:label>
      <skos:definition>A company over which the Incorporated Company has some degree of control by way of ownership of voting shares.</skos:definition>
      <skos:editorialNote>Other means of control exist and are not part of this defined term.</skos:editorialNote>
      <rdfs:subClassOf rdf:resource="http://www.omg.org/spec/EDMC-SR/BE/OwnershipAndControl/ControlParties/ControlledParty"/>
   </owl:Class>

   <owl:Class rdf:about="http://www.omg.org/spec/EDMC-SR/BE/OwnershipAndControl/CorporateControl/DomesticUltimateParent">
      <rdfs:label>Domestic Ultimate Parent</rdfs:label>
      <skos:definition>The organization which is recognized as the ultimate parent of the company within the country or jurisdiction of incorporation. This relationship may or may not be present, i.e. in the case of a company which has no parent.</skos:definition>
      <rdfs:subClassOf rdf:resource="http://www.omg.org/spec/EDMC-SR/BE/OwnershipAndControl/ControlParties/MajorityControllingParty"/>
   </owl:Class>

   <owl:Class rdf:about="http://www.omg.org/spec/EDMC-SR/BE/OwnershipAndControl/CorporateControl/GlobalUltimateParent">
      <rdfs:label>Global Ultimate Parent</rdfs:label>
      <skos:definition>The organization which is recognized as the ultimate parent of the company. This relationship may or may not be present, i.e. in the case of a company which has no parent.</skos:definition>
   </owl:Class>

   <owl:Class rdf:about="http://www.omg.org/spec/EDMC-SR/BE/OwnershipAndControl/CorporateControl/JointVenturePartner">
      <rdfs:label>Joint Venture Partner</rdfs:label>
      <skos:definition>A party which has the role of Joint Venture Partner to some venture.</skos:definition>
      <skos:editorialNote>This is part of ongoing work - legal definitions sought.</skos:editorialNote>
      <rdfs:subClassOf rdf:resource="http://www.omg.org/spec/EDMC-SR/BE/OwnershipAndControl/ControlParties/EntityControllingParty"/>
   </owl:Class>

   <owl:Class rdf:about="http://www.omg.org/spec/EDMC-SR/BE/OwnershipAndControl/CorporateControl/NonWhollyOwnedSubsidiary">
      <rdfs:label>Non Wholly Owned Subsidiary</rdfs:label>
      <skos:definition>A subsidiary which is not a wholly owned subsidiary.</skos:definition>
      <skos:editorialNote>Distinction between wholly owned or not, versus what has to be consolidated into accounts.</skos:editorialNote>
      <rdfs:subClassOf rdf:resource="http://www.omg.org/spec/EDMC-SR/BE/OwnershipAndControl/CorporateControl/Subsidiary"/>
   </owl:Class>

   <owl:Class rdf:about="http://www.omg.org/spec/EDMC-SR/BE/OwnershipAndControl/CorporateControl/OverFiftyPercentControlingInterestCompany">
      <rdfs:label>Over Fifty Percent Controling Interest Company</rdfs:label>
      <rdfs:subClassOf rdf:resource="http://www.omg.org/spec/EDMC-SR/BE/OwnershipAndControl/CorporateControl/VotingShareholdingCompany"/>
   </owl:Class>

   <owl:Class rdf:about="http://www.omg.org/spec/EDMC-SR/BE/OwnershipAndControl/CorporateControl/SignificantShareholdingCompany">
      <rdfs:label>Significant Shareholding Company</rdfs:label>
      <skos:definition>A company which owns a significant voting stake in this company but not 50% or more.</skos:definition>
      <rdfs:subClassOf rdf:resource="http://www.omg.org/spec/EDMC-SR/BE/OwnershipAndControl/ControlParties/SignificantControllingInterestParty"/>
   </owl:Class>

   <owl:Class rdf:about="http://www.omg.org/spec/EDMC-SR/BE/OwnershipAndControl/CorporateControl/Subsidiary">
      <rdfs:label>Subsidiary</rdfs:label>
      <rdfs:subClassOf rdf:resource="http://www.omg.org/spec/EDMC-SR/BE/OwnershipAndControl/CorporateControl/ControlledCompany"/>
   </owl:Class>

   <owl:Class rdf:about="http://www.omg.org/spec/EDMC-SR/BE/OwnershipAndControl/CorporateControl/TotalControllingInterestCompany">
      <rdfs:label>Total Controlling Interest Company</rdfs:label>
      <skos:definition>Formal Organization having 100% ownership in the Incorporated Company so owned.</skos:definition>
      <skos:editorialNote>By virtue of holding 100% of the share ownership, the Company Total Owning company also holds 100% of the controlling equity, if there is a difference. Therefore it is both a total owner and a total controlling party. Scope Note: This party is also a Formal Organization (typically but not necessarily a company).</skos:editorialNote>
      <rdfs:subClassOf rdf:resource="http://www.omg.org/spec/EDMC-SR/BE/OwnershipAndControl/ControlParties/TotalOwner"/>
      <rdfs:subClassOf rdf:resource="http://www.omg.org/spec/EDMC-SR/BE/OwnershipAndControl/CorporateControl/OverFiftyPercentControlingInterestCompany"/>
   </owl:Class>

   <owl:Class rdf:about="http://www.omg.org/spec/EDMC-SR/BE/OwnershipAndControl/CorporateControl/VotingShareholder">
      <rdfs:label>Voting Shareholder</rdfs:label>
      <skos:definition>A party owning voting shares in some company limited by the issue of shares.</skos:definition>
      <rdfs:subClassOf rdf:resource="http://www.omg.org/spec/EDMC-SR/BE/OwnershipAndControl/ControlParties/DeJureControllingInterestParty"/>
      <rdfs:subClassOf rdf:resource="http://www.omg.org/spec/EDMC-SR/BE/OwnershipAndControl/CorporateOwnership/Shareholder"/>
   </owl:Class>

   <owl:Class rdf:about="http://www.omg.org/spec/EDMC-SR/BE/OwnershipAndControl/CorporateControl/VotingShareholding">
      <rdfs:label>Voting Shareholding</rdfs:label>
      <skos:definition>The holding of some Voting Share.</skos:definition>
      <rdfs:subClassOf rdf:resource="http://www.omg.org/spec/EDMC-SR/BE/OwnershipAndControl/CorporateOwnership/Shareholding"/>
   </owl:Class>

   <owl:Class rdf:about="http://www.omg.org/spec/EDMC-SR/BE/OwnershipAndControl/CorporateControl/VotingShareholdingCompany">
      <rdfs:label>Voting Shareholding Company</rdfs:label>
      <skos:definition>A Formal Business Organization which holds voting shares in some Incorporated Company.</skos:definition>
      <skos:editorialNote>This Party forms the basis of the parties defined according to specific percentages of ownership. This term itself defines any company which owns any number of voting shares in the other company, whether it is one share or 100%. Terms like Affiliate (for less than or equal to 50%) and Part Owner (for more than 50%) are specializations of this. Additional comments: So far this assumed one vote per share. This is not always the case. Need to figure out what we want to achieve here. Conclusion: it al matters: KYC: Beneficial ownership structure. goes down to 10% for higher risk organizations. Does this represent controlling ownership or legal ownership for controlling of outstanding shares. There are not always concrete answers from regulators. Corp credit - netting agreements, liquidity agreements and such like. The challenge is known al these. If we have every ownership down to 10%, we need to define those below that since they can roll up. For this exercise, we could limit to less than versus more than 50%. Otherwise it turns into a deep black hole. Other answers may be different depending on rol,e geog and reg regime. Liquidity agreements.</skos:editorialNote>
      <rdfs:subClassOf rdf:resource="http://www.omg.org/spec/EDMC-SR/BE/OwnershipAndControl/CorporateControl/VotingShareholder"/>
   </owl:Class>

   <owl:Class rdf:about="http://www.omg.org/spec/EDMC-SR/BE/OwnershipAndControl/CorporateControl/WhollyOwnedSubsidiary">
      <rdfs:label>Wholly Owned Subsidiary</rdfs:label>
   </owl:Class>

   <!--Individuals-->

</rdf:RDF>