<?xml version="1.0" encoding="UTF-8"?>
<rdf:RDF xmlns:xsd="http://www.w3.org/2001/XMLSchema#"
         xmlns:sm="http://www.omg.org/techprocess/ab/SpecificationMetadata/"
         xmlns:fibo-fnd-utl-av="http://www.omg.org/spec/EDMC-FIBO/FND/Utilities/AnnotationVocabulary/"
         xmlns:rdf="http://www.w3.org/1999/02/22-rdf-syntax-ns#"
         xmlns:rdfs="http://www.w3.org/2000/01/rdf-schema#"
         xmlns:owl="http://www.w3.org/2002/07/owl#"
         xmlns:skos="http://www.w3.org/2004/02/skos/core#"
         xmlns:dc="http://purl.org/dc/terms/"
         xml:base="http://www.omg.org/spec/EDMC-SR/BE/OwnershipAndControl/OwnershipParties/">

   <owl:Ontology rdf:about="http://www.omg.org/spec/EDMC-SR/BE/OwnershipAndControl/OwnershipParties/">
      <owl:imports rdf:resource="http://www.omg.org/spec/EDMC-SR/FND/OwnershipAndControl/Control/"/>
      <owl:imports rdf:resource="http://www.omg.org/spec/EDMC-SR/BE/LegalEntities/FormalBusinessOrganizations/"/>
      <owl:imports rdf:resource="http://www.omg.org/spec/EDMC-SR/FND/OwnershipAndControl/Ownership/"/>
   </owl:Ontology>

   <!--Datatypes-->

<!--Object Properties-->

<owl:ObjectProperty rdf:about="http://www.omg.org/spec/EDMC-SR/BE/OwnershipAndControl/OwnershipParties/constitutionalOwnerHoldsAnInterestIn">
      <rdfs:subPropertyOf rdf:resource="http://www.omg.org/spec/EDMC-SR/BE/OwnershipAndControl/OwnershipParties/holdsAnInterestIn"/>
      <rdfs:domain rdf:resource="http://www.omg.org/spec/EDMC-SR/BE/OwnershipAndControl/OwnershipParties/ConstitutionalOwner"/>
      <rdfs:range rdf:resource="http://www.omg.org/spec/EDMC-SR/BE/LegalEntities/FormalBusinessOrganizations/FormallyConstitutedOrganization"/>
   </owl:ObjectProperty>

   <owl:ObjectProperty rdf:about="http://www.omg.org/spec/EDMC-SR/BE/OwnershipAndControl/OwnershipParties/equityIsEquityHeldBy">
      <rdfs:subPropertyOf rdf:resource="http://www.omg.org/spec/EDMC-SR/BE/OwnershipAndControl/OwnershipParties/isEquityHeldBy"/>
      <rdfs:domain rdf:resource="http://www.omg.org/spec/EDMC-SR/FND/Accounting/AccountingEquity/Equity"/>
      <rdfs:range rdf:resource="http://www.omg.org/spec/EDMC-SR/BE/OwnershipAndControl/OwnershipParties/EntityOwner"/>
      <owl:inverseOf rdf:resource="http://www.omg.org/spec/EDMC-SR/BE/OwnershipAndControl/OwnershipParties/holdsEquity"/>
   </owl:ObjectProperty>

   <owl:ObjectProperty rdf:about="http://www.omg.org/spec/EDMC-SR/BE/OwnershipAndControl/OwnershipParties/guaranteeProvidingMemberGuarantees">
      <skos:definition>Guarantee Providing Member provides a formal assurance or promise, esp. that certain conditions shall be fulfilled relating to a product, service, or transaction, in respect of the Body Incorporated by Guarantee.</skos:definition>
      <rdfs:subPropertyOf rdf:resource="http://www.omg.org/spec/EDMC-SR/BE/OwnershipAndControl/OwnershipParties/guarantees"/>
      <rdfs:domain rdf:resource="http://www.omg.org/spec/EDMC-SR/BE/OwnershipAndControl/OwnershipParties/GuaranteeProvidingMember"/>
      <rdfs:range rdf:resource="http://www.omg.org/spec/EDMC-SR/BE/LegalEntities/CorporateBodies/BodyIncorporatedWithGuarantee"/>
   </owl:ObjectProperty>

   <owl:ObjectProperty rdf:about="http://www.omg.org/spec/EDMC-SR/BE/OwnershipAndControl/OwnershipParties/guarantorHasIdentity">
      <skos:definition>The entity which performs the role of the Guarantor.</skos:definition>
      <skos:editorialNote>This is defined as any Contractually Capable Entity, which itself takes the form of a Formal Organization while also being recognized in some jurisdiction as being capable of incurring contractual liabilities (whether or not it is also a Legal Person).</skos:editorialNote>
      <rdfs:subPropertyOf rdf:resource="http://www.edmcouncil.org/spec/EDMC-SR/FND/Relative/PartyExtensions/organizationMemberHasIdentity"/>
      <rdfs:subPropertyOf rdf:resource="http://www.omg.org/spec/EDMC-SR/FND/Parties/Parties/partyInRoleHasIdentity"/>
      <rdfs:domain rdf:resource="http://www.omg.org/spec/EDMC-SR/BE/OwnershipAndControl/OwnershipParties/GuaranteeProvidingMember"/>
      <rdfs:range rdf:resource="http://www.omg.org/spec/EDMC-SR/FND/Parties/Parties/IndependentParty"/>
   </owl:ObjectProperty>

   <owl:ObjectProperty rdf:about="http://www.omg.org/spec/EDMC-SR/BE/OwnershipAndControl/OwnershipParties/investmentEquityIsEquityHelodBy">
      <skos:definition>Investment is invested by a party which, by virtue of holding some equity investment in the entity, has some ownership stake in it.</skos:definition>
      <rdfs:subPropertyOf rdf:resource="http://www.omg.org/spec/EDMC-SR/BE/OwnershipAndControl/OwnershipParties/isEquityHeldBy"/>
      <rdfs:domain rdf:resource="http://www.omg.org/spec/EDMC-SR/BE/OwnershipAndControl/OwnershipParties/InvestmentEquity"/>
      <rdfs:range rdf:resource="http://www.omg.org/spec/EDMC-SR/BE/OwnershipAndControl/OwnershipParties/Investor"/>
   </owl:ObjectProperty>

   <owl:ObjectProperty rdf:about="http://www.omg.org/spec/EDMC-SR/BE/OwnershipAndControl/OwnershipParties/setsOutTermsForInvestmentEquity">
      <skos:definition>The Contract sets out the terms for the Investment Equity in the entity, setting out the rights which are conferred on any investor in that equity.</skos:definition>
      <rdfs:subPropertyOf rdf:resource="http://www.omg.org/spec/EDMC-SR/FND/Agreements/Contracts/definesTermsFor"/>
      <rdfs:domain rdf:resource="http://www.omg.org/spec/EDMC-SR/BE/OwnershipAndControl/OwnershipParties/InvestorContract"/>
      <rdfs:range rdf:resource="http://www.omg.org/spec/EDMC-SR/BE/OwnershipAndControl/OwnershipParties/InvestmentEquity"/>
   </owl:ObjectProperty>

   <owl:ObjectProperty rdf:about="http://www.omg.org/spec/EDMC-SR/BE/OwnershipAndControl/OwnershipParties/investorHoldsAnInterestIn">
      <rdfs:subPropertyOf rdf:resource="http://www.omg.org/spec/EDMC-SR/BE/OwnershipAndControl/OwnershipParties/holdsAnInterestIn"/>
      <rdfs:domain rdf:resource="http://www.omg.org/spec/EDMC-SR/BE/OwnershipAndControl/OwnershipParties/Investor"/>
      <rdfs:range rdf:resource="http://www.omg.org/spec/EDMC-SR/BE/LegalEntities/FormalBusinessOrganizations/FormallyConstitutedOrganization"/>
   </owl:ObjectProperty>

   <owl:ObjectProperty rdf:about="http://www.omg.org/spec/EDMC-SR/BE/OwnershipAndControl/OwnershipParties/confers">
      <skos:definition>The equity confers some controlling interest on the holder of that equity.</skos:definition>
      <rdfs:subPropertyOf rdf:resource="http://www.omg.org/spec/EDMC-SR/FND/Relations/Relations/confers"/>
      <rdfs:domain rdf:resource="http://www.omg.org/spec/EDMC-SR/BE/OwnershipAndControl/OwnershipParties/ControllingEquity"/>
      <rdfs:range rdf:resource="http://www.omg.org/spec/EDMC-SR/FND/OwnershipAndControl/Control/DeJureControl"/>
   </owl:ObjectProperty>

   <owl:ObjectProperty rdf:about="http://www.omg.org/spec/EDMC-SR/BE/OwnershipAndControl/OwnershipParties/guarantees">
      <skos:definition>provide a formal assurance or promise, esp. that certain conditions shall be fulfilled relating to a product, service, or transaction</skos:definition>
      <rdfs:domain rdf:resource="http://www.omg.org/spec/EDMC-SR/FND/Relations/Relations/Thing"/>
      <rdfs:range rdf:resource="http://www.omg.org/spec/EDMC-SR/FND/Relations/Relations/Thing"/>
   </owl:ObjectProperty>

   <owl:ObjectProperty rdf:about="http://www.omg.org/spec/EDMC-SR/BE/OwnershipAndControl/OwnershipParties/hasConstitutionalOwner">
      <skos:definition>links a constitutional interest/position in something (e.g., a formal business organization) to the party that holds or owns it, in whole or in part</skos:definition>
      <skos:editorialNote>Typically this would be share ownership or the holding of partnership equity. Ownership in this "constitutional" sense means that the owner is in some way a member of the organization, as distinct from some outside investor.</skos:editorialNote>
      <rdfs:subPropertyOf rdf:resource="http://www.omg.org/spec/EDMC-SR/BE/OwnershipAndControl/OwnershipParties/entityOwnedBy"/>
      <rdfs:domain rdf:resource="http://www.omg.org/spec/EDMC-SR/BE/LegalEntities/FormalBusinessOrganizations/FormallyConstitutedOrganization"/>
      <rdfs:range rdf:resource="http://www.omg.org/spec/EDMC-SR/BE/OwnershipAndControl/OwnershipParties/ConstitutionalOwner"/>
   </owl:ObjectProperty>

   <owl:ObjectProperty rdf:about="http://www.omg.org/spec/EDMC-SR/BE/OwnershipAndControl/OwnershipParties/hasInvestor">
      <skos:definition>links an investment interest in something (e.g., a formal business organization) to the party that holds or owns it, in whole or in part</skos:definition>
      <rdfs:subPropertyOf rdf:resource="http://www.omg.org/spec/EDMC-SR/BE/OwnershipAndControl/OwnershipParties/entityOwnedBy"/>
      <rdfs:domain rdf:resource="http://www.omg.org/spec/EDMC-SR/BE/LegalEntities/FormalBusinessOrganizations/FormallyConstitutedOrganization"/>
      <rdfs:range rdf:resource="http://www.omg.org/spec/EDMC-SR/BE/OwnershipAndControl/OwnershipParties/Investor"/>
   </owl:ObjectProperty>

   <owl:ObjectProperty rdf:about="http://www.omg.org/spec/EDMC-SR/BE/OwnershipAndControl/OwnershipParties/holdsSomeInvestmentEquity">
      <skos:definition>Some equity held by the investor in the form of investment equity.</skos:definition>
      <skos:editorialNote>This may or may not be reflected in some "constitutional" form of stockholder equity such as shares or general partner equity.</skos:editorialNote>
      <rdfs:subPropertyOf rdf:resource="http://www.omg.org/spec/EDMC-SR/BE/OwnershipAndControl/OwnershipParties/holdsEquity"/>
      <rdfs:domain rdf:resource="http://www.omg.org/spec/EDMC-SR/BE/OwnershipAndControl/OwnershipParties/Investor"/>
      <rdfs:range rdf:resource="http://www.omg.org/spec/EDMC-SR/BE/OwnershipAndControl/OwnershipParties/InvestmentEquity"/>
   </owl:ObjectProperty>

   <owl:ObjectProperty rdf:about="http://www.omg.org/spec/EDMC-SR/BE/OwnershipAndControl/OwnershipParties/holdsSomeStockholderEquity">
      <skos:definition>A Constitutional Owning Party is defined as such by the fact that they hold some portion of the Stockholder Equity in that entity.</skos:definition>
      <rdfs:subPropertyOf rdf:resource="http://www.omg.org/spec/EDMC-SR/BE/OwnershipAndControl/OwnershipParties/holdsEquity"/>
      <rdfs:domain rdf:resource="http://www.omg.org/spec/EDMC-SR/BE/OwnershipAndControl/OwnershipParties/ConstitutionalOwner"/>
      <rdfs:range rdf:resource="http://www.omg.org/spec/EDMC-SR/FND/Accounting/AccountingEquity/StockholdersEquity"/>
   </owl:ObjectProperty>

   <owl:ObjectProperty rdf:about="http://www.omg.org/spec/EDMC-SR/BE/OwnershipAndControl/OwnershipParties/holdsAnInterestIn">
      <skos:definition>links a party to some organization it holds an interest in</skos:definition>
      <rdfs:subPropertyOf rdf:resource="http://www.omg.org/spec/EDMC-SR/FND/OwnershipAndControl/Ownership/owns"/>
      <rdfs:domain rdf:resource="http://www.omg.org/spec/EDMC-SR/BE/OwnershipAndControl/OwnershipParties/EntityOwner"/>
      <rdfs:range rdf:resource="http://www.omg.org/spec/EDMC-SR/BE/LegalEntities/FormalBusinessOrganizations/FormallyConstitutedOrganization"/>
   </owl:ObjectProperty>

   <owl:ObjectProperty rdf:about="http://www.omg.org/spec/EDMC-SR/BE/OwnershipAndControl/OwnershipParties/holdsEquity">
      <skos:definition>links a party to some equity it holds</skos:definition>
      <rdfs:subPropertyOf rdf:resource="http://www.omg.org/spec/EDMC-SR/FND/OwnershipAndControl/Ownership/owns"/>
      <rdfs:domain rdf:resource="http://www.omg.org/spec/EDMC-SR/BE/OwnershipAndControl/OwnershipParties/EntityOwner"/>
      <rdfs:range rdf:resource="http://www.omg.org/spec/EDMC-SR/FND/Accounting/AccountingEquity/Equity"/>
   </owl:ObjectProperty>

   <owl:ObjectProperty rdf:about="http://www.omg.org/spec/EDMC-SR/BE/OwnershipAndControl/OwnershipParties/involvesEntityOwningParty">
      <skos:definition>Entity ownership involves some party which is identified as an Entity Owning Party.</skos:definition>
      <rdfs:subPropertyOf rdf:resource="http://www.omg.org/spec/EDMC-SR/FND/OwnershipAndControl/Ownership/ownershipInvolves"/>
      <rdfs:domain rdf:resource="http://www.omg.org/spec/EDMC-SR/BE/OwnershipAndControl/OwnershipParties/EntityOwnershipContext"/>
      <rdfs:range rdf:resource="http://www.omg.org/spec/EDMC-SR/BE/OwnershipAndControl/OwnershipParties/EntityOwner"/>
   </owl:ObjectProperty>

   <owl:ObjectProperty rdf:about="http://www.omg.org/spec/EDMC-SR/BE/OwnershipAndControl/OwnershipParties/isEquityHeldBy">
      <skos:definition>links some equity to the party that holds it</skos:definition>
      <rdfs:subPropertyOf rdf:resource="http://www.omg.org/spec/EDMC-SR/FND/OwnershipAndControl/Ownership/isOwnedBy"/>
      <rdfs:domain rdf:resource="http://www.w3.org/2002/07/owl#Thing"/>
      <rdfs:range rdf:resource="http://www.omg.org/spec/EDMC-SR/BE/OwnershipAndControl/OwnershipParties/EntityOwner"/>
   </owl:ObjectProperty>

   <owl:ObjectProperty rdf:about="http://www.omg.org/spec/EDMC-SR/BE/OwnershipAndControl/OwnershipParties/entityOwnedBy">
      <rdfs:subPropertyOf rdf:resource="http://www.omg.org/spec/EDMC-SR/FND/OwnershipAndControl/Ownership/isOwnedBy"/>
      <rdfs:domain rdf:resource="http://www.omg.org/spec/EDMC-SR/BE/LegalEntities/FormalBusinessOrganizations/FormallyConstitutedOrganization"/>
      <rdfs:range rdf:resource="http://www.omg.org/spec/EDMC-SR/BE/OwnershipAndControl/OwnershipParties/EntityOwner"/>
      <owl:inverseOf rdf:resource="http://www.omg.org/spec/EDMC-SR/BE/OwnershipAndControl/OwnershipParties/holdsAnInterestIn"/>
   </owl:ObjectProperty>

   <!--Data Properties-->

<!--Annotation Properties-->

<!--Classes-->

<owl:Class rdf:about="http://www.omg.org/spec/EDMC-SR/BE/OwnershipAndControl/OwnershipParties/ConstitutionalOwner">
      <rdfs:label>Constitutional Owner</rdfs:label>
      <skos:definition>A party which owns some equity stake in some entity, which is some part of the formal equity make-up of that entity, such as shares or general partner equity.</skos:definition>
      <rdfs:subClassOf rdf:resource="http://www.omg.org/spec/EDMC-SR/BE/OwnershipAndControl/OwnershipParties/EntityOwner"/>
   </owl:Class>

   <owl:Class rdf:about="http://www.omg.org/spec/EDMC-SR/BE/OwnershipAndControl/OwnershipParties/ControllingEquity">
      <rdfs:label>Controlling Equity</rdfs:label>
      <skos:definition>Equity which brings with it some form of de jure control of the entity in which it represents and interest.</skos:definition>
      <rdfs:subClassOf rdf:resource="http://www.omg.org/spec/EDMC-SR/FND/Accounting/AccountingEquity/StockholdersEquity"/>
   </owl:Class>

   <owl:Class rdf:about="http://www.omg.org/spec/EDMC-SR/BE/OwnershipAndControl/OwnershipParties/EntityOwner">
      <rdfs:label>Entity Owner</rdfs:label>
      <skos:definition>A party having some ownership in some entity.</skos:definition>
      <skos:editorialNote>This is not the same meaning as being some owner of some asset. Rather, this is some party which partakes in the ownership of some kind of entity (a business entity or a legal entity for example) via some mechanism such as the ownership of equity in that entity.</skos:editorialNote>
      <rdfs:subClassOf rdf:resource="http://www.omg.org/spec/EDMC-SR/FND/OwnershipAndControl/Ownership/Owner"/>
   </owl:Class>

   <owl:Class rdf:about="http://www.omg.org/spec/EDMC-SR/BE/OwnershipAndControl/OwnershipParties/EntityOwnershipContext">
      <rdfs:label>Entity Ownership Context</rdfs:label>
      <skos:definition>The context of ownership by some party of an interest in some Formal Organization.</skos:definition>
      <rdfs:subClassOf rdf:resource="http://www.omg.org/spec/EDMC-SR/FND/OwnershipAndControl/Ownership/Ownership"/>
   </owl:Class>

   <owl:Class rdf:about="http://www.omg.org/spec/EDMC-SR/BE/OwnershipAndControl/OwnershipParties/GuaranteeProvidingMember">
      <rdfs:label>Guarantee Providing Member</rdfs:label>
      <skos:definition>An entity which has issued some Guarantee for a body incorporated by the issuance of Guarantees.</skos:definition>
      <skos:editorialNote>This can be any contractually capable entity.</skos:editorialNote>
      <rdfs:subClassOf rdf:resource="http://www.omg.org/spec/EDMC-SR/BE/LegalEntities/FormalBusinessOrganizations/FormalBusinessOrganizationMember"/>
   </owl:Class>

   <owl:Class rdf:about="http://www.omg.org/spec/EDMC-SR/BE/OwnershipAndControl/OwnershipParties/InvestmentEquity">
      <rdfs:label>Investment Equity</rdfs:label>
      <skos:definition>Equity which represents some investment in some entity, but which may or may not take the form of stockholder equity.</skos:definition>
      <skos:editorialNote>Typically an investment into some entity may take the form of shares (issued or privately held), stockholder equity e.g. partnership equity, or it may take the form of some capital amount which is not reflected in stockholder equity. In each case, there would typically be some contractual basis for the investment setting out what controls or other benefits accrue to the investor.</skos:editorialNote>
      <rdfs:subClassOf rdf:resource="http://www.omg.org/spec/EDMC-SR/FND/Accounting/AccountingEquity/Equity"/>
   </owl:Class>

   <owl:Class rdf:about="http://www.omg.org/spec/EDMC-SR/BE/OwnershipAndControl/OwnershipParties/Investor">
      <rdfs:label>Investor</rdfs:label>
      <skos:definition>A party which owns some stake in some organization by way of investment.</skos:definition>
      <skos:editorialNote>This is regardless of whether or not the investor is also a constitutional owner (e.g. shareholder) in the entity.</skos:editorialNote>
   </owl:Class>

   <owl:Class rdf:about="http://www.omg.org/spec/EDMC-SR/BE/OwnershipAndControl/OwnershipParties/InvestorContract">
      <rdfs:label>Investor Contract</rdfs:label>
      <skos:definition>Contract setting out the terms under which some investor invests in the entity and setting out the rights which are conferred on that investor.</skos:definition>
      <rdfs:subClassOf rdf:resource="http://www.omg.org/spec/EDMC-SR/FND/Agreements/Contracts/WrittenContract"/>
   </owl:Class>

   <!--Individuals-->

</rdf:RDF>