<?xml version="1.0" encoding="UTF-8"?>
<!DOCTYPE rdf:RDF [
	<!ENTITY cmns-av "https://www.omg.org/spec/Commons/AnnotationVocabulary/">
	<!ENTITY dct "http://purl.org/dc/terms/">
	<!ENTITY fibo-fbc-fct-rga "https://spec.edmcouncil.org/fibo/ontology/FBC/FunctionalEntities/RegulatoryAgencies/">
	<!ENTITY fibo-fnd-agr-ctr "https://spec.edmcouncil.org/fibo/ontology/FND/Agreements/Contracts/">
	<!ENTITY fibo-fnd-law-jur "https://spec.edmcouncil.org/fibo/ontology/FND/Law/Jurisdiction/">
	<!ENTITY fibo-fnd-law-lcap "https://spec.edmcouncil.org/fibo/ontology/FND/Law/LegalCapacity/">
	<!ENTITY fibo-fnd-org-fm "https://spec.edmcouncil.org/fibo/ontology/FND/Organizations/FormalOrganizations/">
	<!ENTITY fibo-fnd-rel-rel "https://spec.edmcouncil.org/fibo/ontology/FND/Relations/Relations/">
	<!ENTITY fibo-fnd-utl-av "https://spec.edmcouncil.org/fibo/ontology/FND/Utilities/AnnotationVocabulary/">
	<!ENTITY fibo-loan-ln-app "https://spec.edmcouncil.org/fibo/ontology/LOAN/LoansGeneral/LoanApplications/">
	<!ENTITY fibo-loan-ln-ln "https://spec.edmcouncil.org/fibo/ontology/LOAN/LoansGeneral/Loans/">
	<!ENTITY fibo-loan-ln-reg "https://spec.edmcouncil.org/fibo/ontology/LOAN/LoansGeneral/LoansRegulatory/">
	<!ENTITY owl "http://www.w3.org/2002/07/owl#">
	<!ENTITY rdf "http://www.w3.org/1999/02/22-rdf-syntax-ns#">
	<!ENTITY rdfs "http://www.w3.org/2000/01/rdf-schema#">
	<!ENTITY skos "http://www.w3.org/2004/02/skos/core#">
	<!ENTITY xsd "http://www.w3.org/2001/XMLSchema#">
]>
<rdf:RDF xml:base="https://spec.edmcouncil.org/fibo/ontology/LOAN/LoansGeneral/LoansRegulatory/"
	xmlns:cmns-av="https://www.omg.org/spec/Commons/AnnotationVocabulary/"
	xmlns:dct="http://purl.org/dc/terms/"
	xmlns:fibo-fbc-fct-rga="https://spec.edmcouncil.org/fibo/ontology/FBC/FunctionalEntities/RegulatoryAgencies/"
	xmlns:fibo-fnd-agr-ctr="https://spec.edmcouncil.org/fibo/ontology/FND/Agreements/Contracts/"
	xmlns:fibo-fnd-law-jur="https://spec.edmcouncil.org/fibo/ontology/FND/Law/Jurisdiction/"
	xmlns:fibo-fnd-law-lcap="https://spec.edmcouncil.org/fibo/ontology/FND/Law/LegalCapacity/"
	xmlns:fibo-fnd-org-fm="https://spec.edmcouncil.org/fibo/ontology/FND/Organizations/FormalOrganizations/"
	xmlns:fibo-fnd-rel-rel="https://spec.edmcouncil.org/fibo/ontology/FND/Relations/Relations/"
	xmlns:fibo-fnd-utl-av="https://spec.edmcouncil.org/fibo/ontology/FND/Utilities/AnnotationVocabulary/"
	xmlns:fibo-loan-ln-app="https://spec.edmcouncil.org/fibo/ontology/LOAN/LoansGeneral/LoanApplications/"
	xmlns:fibo-loan-ln-ln="https://spec.edmcouncil.org/fibo/ontology/LOAN/LoansGeneral/Loans/"
	xmlns:fibo-loan-ln-reg="https://spec.edmcouncil.org/fibo/ontology/LOAN/LoansGeneral/LoansRegulatory/"
	xmlns:owl="http://www.w3.org/2002/07/owl#"
	xmlns:rdf="http://www.w3.org/1999/02/22-rdf-syntax-ns#"
	xmlns:rdfs="http://www.w3.org/2000/01/rdf-schema#"
	xmlns:skos="http://www.w3.org/2004/02/skos/core#"
	xmlns:xsd="http://www.w3.org/2001/XMLSchema#">
	
	<owl:Ontology rdf:about="https://spec.edmcouncil.org/fibo/ontology/LOAN/LoansGeneral/LoansRegulatory/">
		<rdfs:label xml:lang="en">LoansRegulatory</rdfs:label>
		<dct:abstract>This ontology contains concepts relating to regulatory requirements around loans, including disclosure rights and a small number of regulation-specific concepts. These include definitions of rights conferred on borrowers under consumer protection law, rights to equal treatment and the like.</dct:abstract>
		<dct:license rdf:datatype="&xsd;anyURI">https://opensource.org/licenses/MIT</dct:license>
		<owl:imports rdf:resource="https://spec.edmcouncil.org/fibo/ontology/FBC/FunctionalEntities/RegulatoryAgencies/"/>
		<owl:imports rdf:resource="https://spec.edmcouncil.org/fibo/ontology/FND/Agreements/Contracts/"/>
		<owl:imports rdf:resource="https://spec.edmcouncil.org/fibo/ontology/FND/Law/Jurisdiction/"/>
		<owl:imports rdf:resource="https://spec.edmcouncil.org/fibo/ontology/FND/Law/LegalCapacity/"/>
		<owl:imports rdf:resource="https://spec.edmcouncil.org/fibo/ontology/FND/Organizations/FormalOrganizations/"/>
		<owl:imports rdf:resource="https://spec.edmcouncil.org/fibo/ontology/FND/Relations/Relations/"/>
		<owl:imports rdf:resource="https://spec.edmcouncil.org/fibo/ontology/FND/Utilities/AnnotationVocabulary/"/>
		<owl:imports rdf:resource="https://spec.edmcouncil.org/fibo/ontology/LOAN/LoansGeneral/LoanApplications/"/>
		<owl:imports rdf:resource="https://spec.edmcouncil.org/fibo/ontology/LOAN/LoansGeneral/Loans/"/>
		<owl:imports rdf:resource="https://www.omg.org/spec/Commons/AnnotationVocabulary/"/>
		<owl:versionIRI rdf:resource="https://spec.edmcouncil.org/fibo/ontology/LOAN/LoansGeneral/LoansRegulatory/"/>
		<fibo-fnd-utl-av:hasMaturityLevel rdf:resource="&fibo-fnd-utl-av;Provisional"/>
		<cmns-av:copyright>Copyright (c) 2013-2023 EDM Council, Inc.</cmns-av:copyright>
	</owl:Ontology>
	
	<owl:Class rdf:about="&fibo-loan-ln-reg;BorrowerDataProtectionRequirement">
		<rdfs:subClassOf rdf:resource="&fibo-loan-ln-reg;DataProtectionRequirement"/>
		<rdfs:subClassOf>
			<owl:Restriction>
				<owl:onProperty rdf:resource="&fibo-fnd-rel-rel;governs"/>
				<owl:someValuesFrom rdf:resource="&fibo-loan-ln-reg;ConsumerCreditReferenceAgency"/>
			</owl:Restriction>
		</rdfs:subClassOf>
		<rdfs:label xml:lang="en">borrower data protection requirement</rdfs:label>
	</owl:Class>
	
	<owl:Class rdf:about="&fibo-loan-ln-reg;BorrowerDisclosureRequirement">
		<rdfs:subClassOf rdf:resource="&fibo-loan-ln-reg;DisclosureRequirement"/>
		<rdfs:subClassOf>
			<owl:Restriction>
				<owl:onProperty rdf:resource="&fibo-fnd-rel-rel;confers"/>
				<owl:someValuesFrom rdf:resource="&fibo-loan-ln-reg;ProductDisclosureRight"/>
			</owl:Restriction>
		</rdfs:subClassOf>
		<rdfs:subClassOf>
			<owl:Restriction>
				<owl:onProperty rdf:resource="&fibo-fnd-rel-rel;governs"/>
				<owl:someValuesFrom rdf:resource="&fibo-loan-ln-app;BorrowerAssessment"/>
			</owl:Restriction>
		</rdfs:subClassOf>
		<rdfs:label xml:lang="en">borrower disclosure requirement</rdfs:label>
	</owl:Class>
	
	<owl:Class rdf:about="&fibo-loan-ln-reg;BorrowerRight">
		<rdfs:subClassOf rdf:resource="&fibo-loan-ln-reg;ConsumerRight"/>
		<rdfs:label xml:lang="en">borrower right</rdfs:label>
		<cmns-av:explanatoryNote xml:lang="en">example the right not to have a home reposessed. Example: RESPA Real Estate Setetlement Procedures Act (promulgated by HUD to govern real estate practices and disclosures Provisions of good faith estimate (GFE) of loan settlement costs. GFE would be when you apply - you get a GFE back from the lender telling you what it would cost if you close the loan.</cmns-av:explanatoryNote>
	</owl:Class>
	
	<owl:Class rdf:about="&fibo-loan-ln-reg;ConsumerCreditEqualTreatmentRequirement">
		<rdfs:subClassOf rdf:resource="&fibo-loan-ln-reg;ConsumerCreditRequirement"/>
		<rdfs:subClassOf>
			<owl:Restriction>
				<owl:onProperty rdf:resource="&fibo-fnd-rel-rel;confers"/>
				<owl:someValuesFrom rdf:resource="&fibo-loan-ln-reg;EqualTreatmentRight"/>
			</owl:Restriction>
		</rdfs:subClassOf>
		<rdfs:label xml:lang="en">consumer credit equal treatment requirement</rdfs:label>
	</owl:Class>
	
	<owl:Class rdf:about="&fibo-loan-ln-reg;ConsumerCreditProtectionLaw">
		<rdfs:subClassOf rdf:resource="&fibo-loan-ln-reg;ConsumerProtectionLaw"/>
		<rdfs:label xml:lang="en">consumer credit protection law</rdfs:label>
	</owl:Class>
	
	<owl:Class rdf:about="&fibo-loan-ln-reg;ConsumerCreditReferenceAgency">
		<rdfs:subClassOf rdf:resource="&fibo-fnd-org-fm;FormalOrganization"/>
		<rdfs:label xml:lang="en">consumer credit reference agency</rdfs:label>
		<skos:definition xml:lang="en">Applicable regulations: vary by jurisdiciton. for example, only being allowed ot divulge actual judgements against a party, but not things that are not substantiated by judgements. For example, slow payments which are not covered by some judgement against the party. There will be different regulatory requirments about: 1. What the CR Agency can hold 2. Who they can divulge it to 3. What information they must provide the borrower at his/her request Some of the third thing there is covered in the EU the Data Protection Directive and local acts that implement this.</skos:definition>
	</owl:Class>
	
	<owl:Class rdf:about="&fibo-loan-ln-reg;ConsumerCreditRequirement">
		<rdfs:subClassOf rdf:resource="&fibo-fnd-law-lcap;LegalObligation"/>
		<rdfs:subClassOf>
			<owl:Restriction>
				<owl:onProperty rdf:resource="&fibo-fnd-rel-rel;confers"/>
				<owl:someValuesFrom rdf:resource="&fibo-loan-ln-reg;ConsumerRight"/>
			</owl:Restriction>
		</rdfs:subClassOf>
		<rdfs:subClassOf>
			<owl:Restriction>
				<owl:onProperty rdf:resource="&fibo-loan-ln-reg;overseenBy"/>
				<owl:someValuesFrom rdf:resource="&fibo-loan-ln-reg;ConsumerProtectionAgency"/>
			</owl:Restriction>
		</rdfs:subClassOf>
		<rdfs:label xml:lang="en">consumer credit requirement</rdfs:label>
		<skos:definition xml:lang="en">Requirement set out on the lender about how they must treat the appliction to a loan</skos:definition>
		<cmns-av:explanatoryNote xml:lang="en">e..g being able to see and challenge information about them held by the credit agency or lender. e.g. can&apos;t publish opinions only facts, etc.</cmns-av:explanatoryNote>
	</owl:Class>
	
	<owl:Class rdf:about="&fibo-loan-ln-reg;ConsumerProtectionAgency">
		<rdfs:subClassOf rdf:resource="&fibo-fbc-fct-rga;RegulatoryAgency"/>
		<rdfs:label xml:lang="en">consumer protection agency</rdfs:label>
		<skos:definition xml:lang="en">Some agency tasked with regulating consumer protection in some jurisdiction.</skos:definition>
		<cmns-av:explanatoryNote xml:lang="en">Note that this is consumer protection, and not other regulatory requirements such as systemic risk. an instance of this is the Consumer Financial Protection Bureau in the US. This is wide rthan just lending, but also covers lender rights.</cmns-av:explanatoryNote>
	</owl:Class>
	
	<owl:Class rdf:about="&fibo-loan-ln-reg;ConsumerProtectionLaw">
		<rdfs:subClassOf rdf:resource="&fibo-fnd-law-jur;StatuteLaw"/>
		<rdfs:label xml:lang="en">consumer protection law</rdfs:label>
	</owl:Class>
	
	<owl:Class rdf:about="&fibo-loan-ln-reg;ConsumerRight">
		<rdfs:subClassOf rdf:resource="&fibo-fnd-law-lcap;LegalRight"/>
		<rdfs:label xml:lang="en">consumer right</rdfs:label>
	</owl:Class>
	
	<owl:Class rdf:about="&fibo-loan-ln-reg;CreditReferenceAgencyRequirements">
		<rdfs:label xml:lang="en">credit reference agency requirements</rdfs:label>
		<skos:definition xml:lang="en">REquirements other than data protection, governing what a credit reference agency can or cannot do.</skos:definition>
		<skos:editorialNote xml:lang="en">Example might include legislation about whether a consumer can be given a bad rating for no good reason; must presumably be some audit requirements about how ratings are arrived at (llogically - no one knows of this; may be addressed simply by the indivbidual&apos;s right to see what&apos;s said. Additional right (not in DP): The right to have something struck from the record of the individual. - see sub term here (Right Or Credit Record Correction). Question: are there additional regulations, rights around not being badly assessed, or is the right of correction (and the access to knowledge) all that there is? May also be rights under common law about the information provided to the agencies.</skos:editorialNote>
	</owl:Class>
	
	<owl:Class rdf:about="&fibo-loan-ln-reg;DataProtectionRequirement">
		<rdfs:subClassOf rdf:resource="&fibo-fnd-law-lcap;LegalObligation"/>
		<rdfs:label xml:lang="en">data protection requirement</rdfs:label>
		<skos:definition xml:lang="en">Requirements defining how data about individuals is held. Example is the EU DA directive and laws, which make the data the property of the individual that data is about. Covers - what information i sheld - who information can be divulged to. - the individual&apos;s rights in respect of that information Privacy regulations cover most of this. EU defines &quot;Personal Data&quot; and &quot;Sensitive Personal Data&quot;. For credit reference agencies the latter would be covered. More detail about whether they can divulge facts which are not subject to formal judgements etc.</skos:definition>
	</owl:Class>
	
	<owl:Class rdf:about="&fibo-loan-ln-reg;DisclosureRequirement">
		<rdfs:subClassOf rdf:resource="&fibo-loan-ln-reg;ConsumerCreditRequirement"/>
		<rdfs:label xml:lang="en">disclosure requirement</rdfs:label>
		<skos:definition xml:lang="en">Requirement for disclosure to borrowers or potential borrowers. There are two kinds of disclosure requirement: 1. Disclosure about the information held on the borrower 2. Disclsure about the product.</skos:definition>
	</owl:Class>
	
	<owl:Class rdf:about="&fibo-loan-ln-reg;EqualTreatmentRight">
		<rdfs:subClassOf rdf:resource="&fibo-loan-ln-reg;BorrowerRight"/>
		<rdfs:label xml:lang="en">equal treatment right</rdfs:label>
		<skos:definition xml:lang="en">The right to equal treatment under the law.</skos:definition>
	</owl:Class>
	
	<owl:Class rdf:about="&fibo-loan-ln-reg;GoodFaithEstimate">
		<rdfs:subClassOf rdf:resource="&fibo-loan-ln-reg;LoanProductRepresentations"/>
		<rdfs:label xml:lang="en">good faith estimate</rdfs:label>
		<skos:definition xml:lang="en">GFE - representation by the lender on the costs and implications of settlement (early termination) of the loan.</skos:definition>
		<cmns-av:explanatoryNote xml:lang="en">Provided in a timely way. Also associated with cooling off periods</cmns-av:explanatoryNote>
	</owl:Class>
	
	<owl:Class rdf:about="&fibo-loan-ln-reg;InformationRight">
		<rdfs:subClassOf rdf:resource="&fibo-loan-ln-reg;BorrowerRight"/>
		<rdfs:label xml:lang="en">information right</rdfs:label>
		<skos:definition xml:lang="en">The right to some information in some context, for example when purchasing some product. The right to full and fair disclosure of</skos:definition>
	</owl:Class>
	
	<owl:Class rdf:about="&fibo-loan-ln-reg;LenderRight">
		<rdfs:subClassOf rdf:resource="&fibo-fnd-law-lcap;LegalRight"/>
		<rdfs:label xml:lang="en">lender right</rdfs:label>
		<skos:definition xml:lang="en">Rights on the lender to protect them against loss. furthe rNtoes: Logically, considering the two parties, they both have protecxtion mechanisms. so while the lender has protecxtion mechanisms through mortgage insurance, and the consumer has protextion mechanisms such as good faith estimates. also the agencies (see Consumer Protection Agency), an instance of which is the CFPB in the US (just set up). Lender rights are: - expressed in the Contract Consumer protection develops becaues the contract is written by the potential Lender. So the rights are introcued to rectify the imbalance between the two parties. Same goes for insurance. consumer protection laws (governe dby the relevant consumer protection agency. So the lender protexts itself as it writes th contract AND does the things it needs to do to protext itself, but on the approval process, and with later instruments such as insurance. Interestingly., it is the Borrower who pays for this by paying for credit reports etc. So the borrower protects itself by other mechanisms. Caveat emptor - displaced by regulation (the buyer is protected by regulation). Uberimae Fidae - in the utmost good faith. Mortgage Insurance is an additional means of mitigating the risk, that the lended may have., so if the information assessed is not accurate, or if the borrower&apos;s situation changes for the worse. then the risk rating may go down. So the Mortgage Insurance is a further strategy which mitigates any shortfall in the Lender Righrs that you may have - ie someone guarantees. In the US you can also avoid that by having paid a deposit. PIMI: Principal, Interst and Morgage Insurance. So the Borrower pays towards the MI, esxcept if they have paid a given amount as deposit. there are 2 types of MI: 1. protects the lender in the event of borrower degault 2. Insurance for &quot;Incapacity to pay the mortage&quot; (these can be bought off the shelf - can combine health, unemployment etc.). - this is the Borrower mitigating their own risk. Prevents foreclosure. Similar to general sickness etc. Where the lender charges for MI, the cost is passed onto the Borrower. e.g. if there is a % valuation (e.g. 70% in Aus, 80% in US for example) then no insurance is required.</skos:definition>
	</owl:Class>
	
	<owl:Class rdf:about="&fibo-loan-ln-reg;LoanProductRepresentations">
		<rdfs:subClassOf rdf:resource="&fibo-fnd-agr-ctr;Representation"/>
		<rdfs:label xml:lang="en">loan product representations</rdfs:label>
		<skos:definition xml:lang="en">Representations about the loan product and the appropriateness of this for the borrower.</skos:definition>
		<cmns-av:explanatoryNote xml:lang="en">Covers responsible lending, consumer credit laws. See Aus Consumer Creti; US Reg Z and so on. In detail, this will include things like the representations about rates of interest, what people can or can&apos;t say when offering a product to a customer. Reg Z: Promoting the informed use of consumer credit by .. implictions and cost Also right to cancel a lien on a consumer&apos;s dwelling.</cmns-av:explanatoryNote>
	</owl:Class>
	
	<owl:Class rdf:about="&fibo-loan-ln-reg;LoanRegulatoryRequirement">
		<rdfs:subClassOf rdf:resource="&fibo-fnd-law-lcap;LegalObligation"/>
		<rdfs:subClassOf>
			<owl:Restriction>
				<owl:onProperty rdf:resource="&fibo-fbc-fct-rga;regulates"/>
				<owl:someValuesFrom rdf:resource="&fibo-loan-ln-ln;Loan"/>
			</owl:Restriction>
		</rdfs:subClassOf>
		<rdfs:subClassOf>
			<owl:Restriction>
				<owl:onProperty rdf:resource="&fibo-fnd-rel-rel;isMandatedBy"/>
				<owl:someValuesFrom rdf:resource="&fibo-loan-ln-reg;ConsumerCreditProtectionLaw"/>
			</owl:Restriction>
		</rdfs:subClassOf>
		<rdfs:subClassOf>
			<owl:Restriction>
				<owl:onProperty rdf:resource="&fibo-loan-ln-reg;administeredBy"/>
				<owl:someValuesFrom rdf:resource="&fibo-fbc-fct-rga;RegulatoryAgency"/>
			</owl:Restriction>
		</rdfs:subClassOf>
		<rdfs:label xml:lang="en">loan regulatory requirement</rdfs:label>
		<skos:definition xml:lang="en">A regulatory requirement defined in regulations by a comsumer credit act or other legislation.</skos:definition>
		<cmns-av:explanatoryNote xml:lang="en">Presence of a loan regulatory requirement associated with a loan indicates that the loan is regulated by the UK Consumer credit act or the equivalent in continental Europe.</cmns-av:explanatoryNote>
	</owl:Class>
	
	<owl:Class rdf:about="&fibo-loan-ln-reg;ProductDisclosureRequirement">
		<rdfs:subClassOf rdf:resource="&fibo-loan-ln-reg;DisclosureRequirement"/>
		<rdfs:subClassOf>
			<owl:Restriction>
				<owl:onProperty rdf:resource="&fibo-fnd-rel-rel;governs"/>
				<owl:someValuesFrom rdf:resource="&fibo-loan-ln-reg;GoodFaithEstimate"/>
			</owl:Restriction>
		</rdfs:subClassOf>
		<rdfs:subClassOf>
			<owl:Restriction>
				<owl:onProperty rdf:resource="&fibo-fnd-rel-rel;governs"/>
				<owl:someValuesFrom rdf:resource="&fibo-loan-ln-reg;LoanProductRepresentations"/>
			</owl:Restriction>
		</rdfs:subClassOf>
		<rdfs:label xml:lang="en">product disclosure requirement</rdfs:label>
		<skos:definition xml:lang="en">A requirement governing what representations can be made about a product, as it affects the consumer.</skos:definition>
		<cmns-av:explanatoryNote xml:lang="en">There are also rules which encompass limitations on how you might attach loans and liens to principle dwellings, e.g. when or whether you can foreclose on someone&apos;s principal dwelling with impunity; what rights the consumer has - this last will be a separate kind of regulation.</cmns-av:explanatoryNote>
	</owl:Class>
	
	<owl:Class rdf:about="&fibo-loan-ln-reg;ProductDisclosureRight">
		<rdfs:subClassOf rdf:resource="&fibo-loan-ln-reg;InformationRight"/>
		<rdfs:label xml:lang="en">product disclosure right</rdfs:label>
		<skos:definition xml:lang="en">The right to information about products at the point of purchasing these.</skos:definition>
		<cmns-av:explanatoryNote xml:lang="en">Includes retail, insurance and financial product disclosures</cmns-av:explanatoryNote>
	</owl:Class>
	
	<owl:Class rdf:about="&fibo-loan-ln-reg;RegB">
		<rdfs:subClassOf rdf:resource="&fibo-loan-ln-reg;ConsumerCreditEqualTreatmentRequirement"/>
		<rdfs:subClassOf rdf:resource="&fibo-loan-ln-reg;DisclosureRequirement"/>
		<rdfs:label xml:lang="en">reg b</rdfs:label>
		<skos:definition xml:lang="en">US regulation concerning &quot;Equal credit opportunity act&quot; Electronic delivery of disclosures</skos:definition>
		<cmns-av:explanatoryNote xml:lang="en">Timing and delivery of electronic disclosures. Applications must have equal opportunity to follow. All applications for credit to be evaluated equally and not discriminiated against. This is disclosures about the Borrower.</cmns-av:explanatoryNote>
	</owl:Class>
	
	<owl:Class rdf:about="&fibo-loan-ln-reg;RegZ">
		<rdfs:subClassOf rdf:resource="&fibo-loan-ln-reg;ProductDisclosureRequirement"/>
		<rdfs:label xml:lang="en">reg z</rdfs:label>
		<skos:definition xml:lang="en">US Fed regulation &quot;Truth in Lending Act&quot; uniform standards for electronic delivery of disclosures</skos:definition>
		<cmns-av:explanatoryNote xml:lang="en">Creditors may delivery disclosures electronic if they obtain consumer&apos;s consent. Also relate to international, and foreign languages. This is disclosures about the Product.</cmns-av:explanatoryNote>
	</owl:Class>
	
	<owl:Class rdf:about="&fibo-loan-ln-reg;RightOfCreditRecordCorrection">
		<rdfs:subClassOf rdf:resource="&fibo-loan-ln-reg;CreditReferenceAgencyRequirements"/>
		<rdfs:label xml:lang="en">right of credit record correction</rdfs:label>
		<skos:definition xml:lang="en">The right to have a credit record corrected.</skos:definition>
	</owl:Class>
	
	<owl:ObjectProperty rdf:about="&fibo-loan-ln-reg;administeredBy">
		<rdfs:label xml:lang="en">administered by</rdfs:label>
		<rdfs:domain rdf:resource="&fibo-loan-ln-reg;LoanRegulatoryRequirement"/>
		<rdfs:range rdf:resource="&fibo-fbc-fct-rga;RegulatoryAgency"/>
	</owl:ObjectProperty>
	
	<owl:ObjectProperty rdf:about="&fibo-loan-ln-reg;overseenBy">
		<rdfs:label xml:lang="en">overseen by</rdfs:label>
		<rdfs:domain rdf:resource="&fibo-loan-ln-reg;ConsumerCreditRequirement"/>
		<rdfs:range rdf:resource="&fibo-loan-ln-reg;ConsumerProtectionAgency"/>
	</owl:ObjectProperty>
	
	<owl:DatatypeProperty rdf:about="&fibo-loan-ln-reg;requirementActReference">
		<rdfs:label xml:lang="en">requirement act reference</rdfs:label>
		<rdfs:domain rdf:resource="&fibo-loan-ln-reg;LoanRegulatoryRequirement"/>
		<rdfs:range rdf:resource="&xsd;string"/>
	</owl:DatatypeProperty>
	
	<owl:DatatypeProperty rdf:about="&fibo-loan-ln-reg;requirementSectionAndParagraph">
		<rdfs:label xml:lang="en">requirement section and paragraph</rdfs:label>
		<rdfs:domain rdf:resource="&fibo-loan-ln-reg;LoanRegulatoryRequirement"/>
		<rdfs:range rdf:resource="&xsd;string"/>
	</owl:DatatypeProperty>

</rdf:RDF>