<?xml version="1.0" encoding="UTF-8"?>
  
<!DOCTYPE rdf:RDF [
    <!ENTITY fibo-be-le-cb "http://spec.edmcouncil.org/fibo/red/be/legal-entities/corporate-bodies/">
    <!ENTITY fibo-fnd-law-cor "http://spec.edmcouncil.org/fibo/red/fnd/law/legal-core/">
    <!ENTITY fibo-be-le-lp "http://spec.edmcouncil.org/fibo/red/be/legal-entities/legal-persons/">
    <!ENTITY fibo-be-le-fbo "http://spec.edmcouncil.org/fibo/red/be/legal-entities/formal-business-organizations/">
    <!ENTITY fibo-fnd-utl-bt "http://spec.edmcouncil.org/fibo/red/fnd/utilities/business-facing-types/">
    <!ENTITY fibo-fnd-acc-cur "http://spec.edmcouncil.org/fibo/red/fnd/accounting/currency-amount/">
    <!ENTITY fibo-fnd-plc-cty "http://spec.edmcouncil.org/fibo/red/fnd/places/countries/">
    <!ENTITY fibo-fnd-law-jur "http://spec.edmcouncil.org/fibo/red/fnd/law/jurisdictions/">
    <!ENTITY fibo-fnd-acc-aeq "http://spec.edmcouncil.org/fibo/red/fnd/accounting/accounting-equity/">
    <!ENTITY fibo-fnd-rel-rel "http://spec.edmcouncil.org/fibo/red/fnd/relations/relations/">
]>

<rdf:RDF xmlns:xsd="http://www.w3.org/2001/XMLSchema#"
         xmlns:sm="http://www.omg.org/techprocess/ab/SpecificationMetadata/"
         xmlns:xs="http://www.w3.org/2001/XMLSchema"
         xmlns:fibo-fnd-utl-av="http://www.omg.org/spec/EDMC-FIBO/FND/Utilities/AnnotationVocabulary/"
         xmlns:rdf="http://www.w3.org/1999/02/22-rdf-syntax-ns#"
         xmlns:rdfs="http://www.w3.org/2000/01/rdf-schema#"
         xmlns:owl="http://www.w3.org/2002/07/owl#"
         xmlns:skos="http://www.w3.org/2004/02/skos/core#"
         xmlns:dc="http://purl.org/dc/terms/"
         xml:base="http://spec.edmcouncil.org/fibo/red/be/legal-entities/corporate-bodies/">

   <owl:Ontology rdf:about="http://spec.edmcouncil.org/fibo/red/be/legal-entities/corporate-bodies/">
      <owl:imports rdf:resource="http://spec.edmcouncil.org/fibo/red/fnd/law/legal-core/"/>
      <owl:imports rdf:resource="http://spec.edmcouncil.org/fibo/red/be/legal-entities/legal-persons/"/>
      <owl:imports rdf:resource="http://spec.edmcouncil.org/fibo/red/be/legal-entities/formal-business-organizations/"/>
      <owl:imports rdf:resource="http://spec.edmcouncil.org/fibo/red/fnd/utilities/business-facing-types/"/>
      <owl:imports rdf:resource="http://spec.edmcouncil.org/fibo/red/fnd/accounting/currency-amount/"/>
      <owl:imports rdf:resource="http://spec.edmcouncil.org/fibo/red/fnd/places/countries/"/>
      <owl:imports rdf:resource="http://spec.edmcouncil.org/fibo/red/fnd/law/jurisdictions/"/>
      <owl:imports rdf:resource="http://spec.edmcouncil.org/fibo/red/fnd/accounting/accounting-equity/"/>
      <owl:imports rdf:resource="http://spec.edmcouncil.org/fibo/red/fnd/relations/relations/"/>
   </owl:Ontology>


  <!--
    ///////////////////////////////////////////////////////////////////////////////////////
    //
    // Datatypes
    //
    ///////////////////////////////////////////////////////////////////////////////////////
    -->



  <!--
    ///////////////////////////////////////////////////////////////////////////////////////
    //
    // Object Properties
    //
    ///////////////////////////////////////////////////////////////////////////////////////
    -->


<owl:ObjectProperty rdf:about="&fibo-be-le-cb;bodyCorporateIsConstitutedBy">
      <rdfs:label>body corporate is constituted by</rdfs:label>
      <rdfs:subPropertyOf rdf:resource="&fibo-be-le-cb;isConstitutedBy"/>
      <rdfs:domain rdf:resource="&fibo-be-le-cb;BodyCorporate"/>
      <rdfs:range rdf:resource="&fibo-be-le-cb;InstrumentOfIncorporation"/>
   </owl:ObjectProperty>

   <owl:ObjectProperty rdf:about="&fibo-be-le-cb;bodyIncorporatedWithGuaranteeIsGovernedBy">
      <rdfs:label>body incorporated with guarantee is governed by</rdfs:label>
      <skos:definition>The company is governed by some formal agreement between the principals.</skos:definition>
      <rdfs:subPropertyOf rdf:resource="&fibo-be-le-fbo;formallyConstitutedOrganizationIsGovernedBy"/>
      <rdfs:domain rdf:resource="&fibo-be-le-cb;BodyIncorporatedWithGuarantee"/>
      <rdfs:range rdf:resource="&fibo-be-le-cb;BodyLimitedByGuaranteePrincipalsAgreement"/>
   </owl:ObjectProperty>

   <owl:ObjectProperty rdf:about="&fibo-be-le-cb;guaranteeIsProvidedBy">
      <rdfs:label>guarantee is provided by</rdfs:label>
      <rdfs:subPropertyOf rdf:resource="&fibo-fnd-rel-rel;isProvidedBy"/>
      <rdfs:domain rdf:resource="&fibo-be-le-cb;IncorporationGuarantee"/>
      <rdfs:range rdf:resource="&fibo-fnd-rel-rel;Thing"/>
   </owl:ObjectProperty>

   <owl:ObjectProperty rdf:about="&fibo-be-le-cb;incorporationGuaranteeHasNotionalAmount">
      <rdfs:label>incorporation guarantee has notional amount</rdfs:label>
      <rdfs:subPropertyOf rdf:resource="&fibo-fnd-acc-cur;hasNotionalAmount"/>
      <rdfs:domain rdf:resource="&fibo-be-le-cb;IncorporationGuarantee"/>
      <rdfs:range rdf:resource="&fibo-fnd-acc-cur;MonetaryAmount"/>
   </owl:ObjectProperty>

   <owl:ObjectProperty rdf:about="&fibo-be-le-cb;instrumentOfIncorporationIsGovernedBy">
      <rdfs:label>instrument of incorporation is governed by</rdfs:label>
      <skos:definition>The legal jurisdiction under which the Instrument of Incorporation has standing.</skos:definition>
      <rdfs:subPropertyOf rdf:resource="&fibo-fnd-rel-rel;isGoverneBy"/>
      <rdfs:domain rdf:resource="&fibo-be-le-cb;InstrumentOfIncorporation"/>
      <rdfs:range rdf:resource="&fibo-fnd-law-jur;Jurisdiction"/>
   </owl:ObjectProperty>

   <owl:ObjectProperty rdf:about="&fibo-be-le-cb;isConstitutedBy">
      <rdfs:label>is constituted by</rdfs:label>
      <skos:definition>The instrument by which the entity is incorporated.</skos:definition>
      <rdfs:domain rdf:resource="&fibo-be-le-cb;BodyCorporate"/>
      <rdfs:range rdf:resource="&fibo-fnd-law-cor;Constitution"/>
   </owl:ObjectProperty>

   <owl:ObjectProperty rdf:about="&fibo-be-le-cb;isDomiciledIn">
      <rdfs:label>is domiciled in</rdfs:label>
      <skos:definition>The country in which the Body Corporate is officially domiciled.</skos:definition>
      <rdfs:domain rdf:resource="&fibo-be-le-cb;BodyCorporate"/>
      <rdfs:range rdf:resource="&fibo-fnd-plc-cty;Country"/>
   </owl:ObjectProperty>

   <owl:ObjectProperty rdf:about="&fibo-be-le-cb;isIncorporatedIn">
      <rdfs:label>is incorporated in</rdfs:label>
      <skos:definition>The legal jurisdiction under which the legal entity is incorporated.</skos:definition>
      <rdfs:domain rdf:resource="&fibo-be-le-cb;BodyCorporate"/>
      <rdfs:range rdf:resource="&fibo-fnd-law-jur;Jurisdiction"/>
   </owl:ObjectProperty>

   <owl:ObjectProperty rdf:about="&fibo-be-le-cb;issuesEquity">
      <rdfs:label>issues equity</rdfs:label>
      <skos:definition>The Body Incorporated by Equity is incorporated through the issuance of some Issued Equity, which is a form of Stockholder Equity.</skos:definition>
      <rdfs:subPropertyOf rdf:resource="&fibo-be-le-fbo;hasEquity"/>
      <rdfs:domain rdf:resource="&fibo-be-le-cb;BodyIncorporatedWithEquity"/>
      <rdfs:range rdf:resource="&fibo-fnd-acc-aeq;IssuedEquity"/>
   </owl:ObjectProperty>


  <!--
    ///////////////////////////////////////////////////////////////////////////////////////
    //
    // Data Properties
    //
    ///////////////////////////////////////////////////////////////////////////////////////
    -->


<owl:DatatypeProperty rdf:about="&fibo-be-le-cb;hasLegalName">
      <rdfs:label>has legal name</rdfs:label>
      <rdfs:range rdf:resource="&fibo-fnd-utl-bt;text"/>
   </owl:DatatypeProperty>

   <owl:DatatypeProperty rdf:about="&fibo-be-le-cb;instrumentURI">
      <rdfs:label>instrument u r i</rdfs:label>
      <skos:definition>The URI of the Instrument of Incorporation.</skos:definition>
      <rdfs:range rdf:resource="&fibo-fnd-utl-bt;URI"/>
   </owl:DatatypeProperty>


  <!--
    ///////////////////////////////////////////////////////////////////////////////////////
    //
    // Annotation Properties
    //
    ///////////////////////////////////////////////////////////////////////////////////////
    -->



  <!--
    ///////////////////////////////////////////////////////////////////////////////////////
    //
    // Classes
    //
    ///////////////////////////////////////////////////////////////////////////////////////
    -->


<owl:Class rdf:about="&fibo-be-le-cb;BodyCorporate">
      <rdfs:label>body corporate</rdfs:label>
      <skos:definition>Any formal organization which can incur liability and can be sued at law and which is not an individual human being.</skos:definition>
      <rdfs:subClassOf rdf:resource="&fibo-be-le-fbo;FormallyConstitutedOrganization"/>
      <rdfs:subClassOf rdf:resource="&fibo-be-le-lp;JudicialPerson"/>
   </owl:Class>

   <owl:Class rdf:about="&fibo-be-le-cb;BodyIncorporatedThroughAgreement">
      <rdfs:label>body incorporated through agreement</rdfs:label>
      <skos:definition>A body with legal personhood, incorporated through some agreement among the principals, and without equity or guarantee instruments which would isolate the principals from liability.</skos:definition>
      <rdfs:subClassOf rdf:resource="&fibo-be-le-cb;BodyCorporate"/>
   </owl:Class>

   <owl:Class rdf:about="&fibo-be-le-cb;BodyIncorporatedWithEquity">
      <rdfs:label>body incorporated with equity</rdfs:label>
      <skos:definition>A body corporate which is incorporated by means of the issuance of equity.</skos:definition>
   </owl:Class>

   <owl:Class rdf:about="&fibo-be-le-cb;BodyIncorporatedWithGuarantee">
      <rdfs:label>body incorporated with guarantee</rdfs:label>
   </owl:Class>

   <owl:Class rdf:about="&fibo-be-le-cb;BodyLimitedByGuaranteePrincipalsAgreement">
      <rdfs:label>body limited by guarantee principals agreement</rdfs:label>
      <skos:definition>The formal agreement between the principals of a Body Limited by Guarantee.</skos:definition>
      <rdfs:subClassOf rdf:resource="&fibo-be-le-fbo;OrganizationCoveringAgreement"/>
   </owl:Class>

   <owl:Class rdf:about="&fibo-be-le-cb;CompanyIncorporatedByGuarantee">
      <rdfs:label>company incorporated by guarantee</rdfs:label>
      <rdfs:subClassOf rdf:resource="&fibo-be-le-cb;BodyIncorporatedWithGuarantee"/>
   </owl:Class>

   <owl:Class rdf:about="&fibo-be-le-cb;IncorporationGuarantee">
      <rdfs:label>incorporation guarantee</rdfs:label>
      <skos:definition>A guarantee which is part of the means by which some incorporated entity is incorporated by guarantee.</skos:definition>
      <rdfs:subClassOf rdf:resource="&fibo-fnd-law-cor;Constitution"/>
   </owl:Class>

   <owl:Class rdf:about="&fibo-be-le-cb;InstrumentOfIncorporation">
      <rdfs:label>instrument of incorporation</rdfs:label>
      <skos:definition>Some legal instrument by which some legal entity which is not a natural person is made to exist.</skos:definition>
   </owl:Class>


  <!--
    ///////////////////////////////////////////////////////////////////////////////////////
    //
    // Individuals
    //
    ///////////////////////////////////////////////////////////////////////////////////////
    -->


</rdf:RDF>