<?xml version="1.0" encoding="UTF-8"?>
<rdf:RDF xmlns:xsd="http://www.w3.org/2001/XMLSchema#"
         xmlns:sm="http://www.omg.org/techprocess/ab/SpecificationMetadata/"
         xmlns:fibo-fnd-utl-av="http://www.omg.org/spec/EDMC-FIBO/FND/Utilities/AnnotationVocabulary/"
         xmlns:rdf="http://www.w3.org/1999/02/22-rdf-syntax-ns#"
         xmlns:rdfs="http://www.w3.org/2000/01/rdf-schema#"
         xmlns:owl="http://www.w3.org/2002/07/owl#"
         xmlns:skos="http://www.w3.org/2004/02/skos/core#"
         xmlns:dc="http://purl.org/dc/terms/"
         xml:base="http://www.edmcouncil.org/spec/EDMC-SR/FND/Publications/Conventions/">

   <owl:Ontology rdf:about="http://www.edmcouncil.org/spec/EDMC-SR/FND/Publications/Conventions/">
      <owl:imports rdf:resource="http://www.edmcouncil.org/spec/EDMC-SR/FND/Publications/Standards/"/>
   </owl:Ontology>

   <!--Datatypes-->

<!--Object Properties-->

<owl:ObjectProperty rdf:about="http://www.edmcouncil.org/spec/EDMC-SR/FND/Publications/Conventions/industryModelConventionDefinedBy">
      <skos:definition>Some Industry Association which defines the convention.</skos:definition>
      <skos:editorialNote>This relationship exists in order to be able to define conventions which do not have the formal standards but which are maintained in some way by some industry association, for example by publication of a website.</skos:editorialNote>
      <rdfs:subPropertyOf rdf:resource="http://www.edmcouncil.org/spec/EDMC-SR/FND/Publications/Conventions/conventionPublishedBy"/>
      <rdfs:domain rdf:resource="http://www.edmcouncil.org/spec/EDMC-SR/FND/Publications/Conventions/IndustryModelConvention"/>
      <rdfs:range rdf:resource="http://www.edmcouncil.org/spec/EDMC-SR/FND/Publications/Standards/IndustryAssociation"/>
   </owl:ObjectProperty>

   <owl:ObjectProperty rdf:about="http://www.edmcouncil.org/spec/EDMC-SR/FND/Publications/Conventions/standardSetBy">
      <skos:definition>A Standards Body which acts as the setter of the Standard.</skos:definition>
      <skos:editorialNote>This is the case whereby the entity which sets the standard is one which is specifically set up for the purpose of setting standards.</skos:editorialNote>
      <rdfs:subPropertyOf rdf:resource="http://www.edmcouncil.org/spec/EDMC-SR/FND/Publications/Standards/standardSetBy"/>
      <rdfs:subPropertyOf rdf:resource="http://www.edmcouncil.org/spec/EDMC-SR/FND/Publications/Standards/standardsSetterIdentity"/>
      <rdfs:domain rdf:resource="http://www.edmcouncil.org/spec/EDMC-SR/FND/Publications/Standards/TechnicalStandard"/>
      <rdfs:range rdf:resource="http://www.edmcouncil.org/spec/EDMC-SR/FND/Publications/Standards/StandardsBody"/>
   </owl:ObjectProperty>

   <owl:ObjectProperty rdf:about="http://www.edmcouncil.org/spec/EDMC-SR/FND/Publications/Conventions/conventionPublishedBy">
      <skos:definition>Unlike other published information, a convention is deemed to be in the public domain and therefore published, but there is no reason for the Publisher to be known or to exist as such.</skos:definition>
      <rdfs:subPropertyOf rdf:resource="http://www.edmcouncil.org/spec/EDMC-SR/FND/Publications/Publications/publishedBy"/>
      <rdfs:domain rdf:resource="http://www.edmcouncil.org/spec/EDMC-SR/FND/Publications/Conventions/Convention"/>
      <rdfs:range rdf:resource="http://www.edmcouncil.org/spec/EDMC-SR/FND/Publications/Publications/Publisher"/>
   </owl:ObjectProperty>

   <!--Data Properties-->

<!--Annotation Properties-->

<!--Classes-->

<owl:Class rdf:about="http://www.edmcouncil.org/spec/EDMC-SR/FND/Publications/Conventions/ISOStandard">
      <rdfs:label>ISO Standard</rdfs:label>
      <skos:definition>A standard published and mandated by the International Standards Organisation (ISO).</skos:definition>
      <rdfs:subClassOf rdf:resource="http://www.edmcouncil.org/spec/EDMC-SR/FND/Publications/Standards/TechnicalStandard"/>
   </owl:Class>

   <owl:Class rdf:about="http://www.edmcouncil.org/spec/EDMC-SR/FND/Publications/Conventions/IndustryModelConvention">
      <rdfs:label>Industry Model Convention</rdfs:label>
      <skos:definition>Standard conventions which exist in the public domain but are not enshrined in an existing ISO Standard are defined in this model and published as such.</skos:definition>
      <rdfs:subClassOf rdf:resource="http://www.edmcouncil.org/spec/EDMC-SR/FND/Publications/Conventions/Convention"/>
   </owl:Class>

   <owl:Class rdf:about="http://www.edmcouncil.org/spec/EDMC-SR/FND/Publications/Conventions/Convention">
      <rdfs:label>Convention</rdfs:label>
      <skos:definition>The way something is usually done.</skos:definition>
      <rdfs:subClassOf rdf:resource="http://www.edmcouncil.org/spec/EDMC-SR/FND/Publications/Publications/PublishedInformation"/>
   </owl:Class>

   <!--Individuals-->

</rdf:RDF>