<?xml version="1.0" encoding="UTF-8"?>
  
<!DOCTYPE rdf:RDF [
    <!ENTITY fibo-fnd-pub-pub "http://spec.edmcouncil.org/fibo/red/fnd/publications/publications/">
    <!ENTITY fibo-fnd-info-info "http://spec.edmcouncil.org/fibo/red/fnd/information/info-core/">
    <!ENTITY fibo-fnd-pty-rl "http://spec.edmcouncil.org/fibo/red/fnd/parties/roles/">
    <!ENTITY fibo-fnd-rel-rel "http://spec.edmcouncil.org/fibo/red/fnd/relations/relations/">
    <!ENTITY fibo-fnd-utl-bt "http://spec.edmcouncil.org/fibo/red/fnd/utilities/business-facing-types/">
    <!ENTITY fibo-be-le-fbo "http://spec.edmcouncil.org/fibo/red/be/legal-entities/formal-business-organizations/">
]>

<rdf:RDF xmlns:xsd="http://www.w3.org/2001/XMLSchema#"
         xmlns:sm="http://www.omg.org/techprocess/ab/SpecificationMetadata/"
         xmlns:xs="http://www.w3.org/2001/XMLSchema"
         xmlns:fibo-fnd-utl-av="http://www.omg.org/spec/EDMC-FIBO/FND/Utilities/AnnotationVocabulary/"
         xmlns:rdf="http://www.w3.org/1999/02/22-rdf-syntax-ns#"
         xmlns:rdfs="http://www.w3.org/2000/01/rdf-schema#"
         xmlns:owl="http://www.w3.org/2002/07/owl#"
         xmlns:skos="http://www.w3.org/2004/02/skos/core#"
         xmlns:dc="http://purl.org/dc/terms/"
         xml:base="http://spec.edmcouncil.org/fibo/red/fnd/publications/publications/">

   <owl:Ontology rdf:about="http://spec.edmcouncil.org/fibo/red/fnd/publications/publications/">
      <owl:imports rdf:resource="http://spec.edmcouncil.org/fibo/red/fnd/information/info-core/"/>
      <owl:imports rdf:resource="http://spec.edmcouncil.org/fibo/red/fnd/parties/roles/"/>
      <owl:imports rdf:resource="http://spec.edmcouncil.org/fibo/red/fnd/relations/relations/"/>
      <owl:imports rdf:resource="http://spec.edmcouncil.org/fibo/red/fnd/utilities/business-facing-types/"/>
      <owl:imports rdf:resource="http://spec.edmcouncil.org/fibo/red/be/legal-entities/formal-business-organizations/"/>
   </owl:Ontology>


  <!--
    ///////////////////////////////////////////////////////////////////////////////////////
    //
    // Datatypes
    //
    ///////////////////////////////////////////////////////////////////////////////////////
    -->



  <!--
    ///////////////////////////////////////////////////////////////////////////////////////
    //
    // Object Properties
    //
    ///////////////////////////////////////////////////////////////////////////////////////
    -->


<owl:ObjectProperty rdf:about="&fibo-fnd-pub-pub;publisherIdentity">
      <rdfs:label>publisher identity</rdfs:label>
      <skos:definition>A publisher of information may be identified as any Business Entity, including for example specialized publishing house, ratings agency, standards body and so on.</skos:definition>
      <rdfs:subPropertyOf rdf:resource="&fibo-fnd-rel-rel;hasIdentity"/>
      <rdfs:domain rdf:resource="&fibo-fnd-pub-pub;Publisher"/>
      <rdfs:range rdf:resource="&fibo-be-le-fbo;FormallyConstitutedOrganization"/>
   </owl:ObjectProperty>

   <owl:ObjectProperty rdf:about="&fibo-fnd-pub-pub;isAbout">
      <rdfs:label>is about</rdfs:label>
      <skos:definition>The subject matter of the published information.</skos:definition>
      <rdfs:subPropertyOf rdf:resource="&fibo-fnd-info-info;isAbout"/>
      <rdfs:domain rdf:resource="&fibo-fnd-pub-pub;PublishedInformation"/>
      <rdfs:range rdf:resource="http://www.w3.org/2002/07/owl#Thing"/>
   </owl:ObjectProperty>

   <owl:ObjectProperty rdf:about="&fibo-fnd-pub-pub;publishedBy">
      <rdfs:label>published by</rdfs:label>
      <skos:definition>The organization which makes this information available.</skos:definition>
      <rdfs:subPropertyOf rdf:resource="&fibo-fnd-rel-rel;isProvidedBy"/>
      <rdfs:domain rdf:resource="&fibo-fnd-pub-pub;PublishedInformation"/>
      <rdfs:range rdf:resource="&fibo-fnd-pub-pub;Publisher"/>
   </owl:ObjectProperty>


  <!--
    ///////////////////////////////////////////////////////////////////////////////////////
    //
    // Data Properties
    //
    ///////////////////////////////////////////////////////////////////////////////////////
    -->


<owl:DatatypeProperty rdf:about="&fibo-fnd-pub-pub;uRL">
      <rdfs:label>u r l</rdfs:label>
      <skos:definition>The URL of the web page.</skos:definition>
      <rdfs:range rdf:resource="&fibo-fnd-utl-bt;URI"/>
   </owl:DatatypeProperty>

   <owl:DatatypeProperty rdf:about="&fibo-fnd-pub-pub;brandName">
      <rdfs:label>brand name</rdfs:label>
      <skos:definition>The name of marque by which the publisher is identified in its publications. This may or may not be identical to the legal name or the Trading As name, but represents a separate semantic. Usually to be found on book jackets, press releases etc.</skos:definition>
      <rdfs:range rdf:resource="&fibo-fnd-utl-bt;text"/>
   </owl:DatatypeProperty>


  <!--
    ///////////////////////////////////////////////////////////////////////////////////////
    //
    // Annotation Properties
    //
    ///////////////////////////////////////////////////////////////////////////////////////
    -->



  <!--
    ///////////////////////////////////////////////////////////////////////////////////////
    //
    // Classes
    //
    ///////////////////////////////////////////////////////////////////////////////////////
    -->


<owl:Class rdf:about="&fibo-fnd-pub-pub;WebPage">
      <rdfs:label>web page</rdfs:label>
      <skos:definition>A document published on the World Wide Web and accessible via a Universal Resource Locator.</skos:definition>
      <rdfs:subClassOf rdf:resource="&fibo-fnd-info-info;Document"/>
   </owl:Class>

   <owl:Class rdf:about="&fibo-fnd-pub-pub;PublishedInformation">
      <rdfs:label>published information</rdfs:label>
      <rdfs:subClassOf rdf:resource="&fibo-fnd-info-info;Information"/>
   </owl:Class>

   <owl:Class rdf:about="&fibo-fnd-pub-pub;Publisher">
      <rdfs:label>publisher</rdfs:label>
      <skos:definition>An organization (such as a publishing house) which makes information. available.</skos:definition>
      <rdfs:subClassOf rdf:resource="&fibo-fnd-pty-rl;AgentInRole"/>
   </owl:Class>

   <owl:Class rdf:about="&fibo-fnd-pub-pub;PublishingHouse">
      <rdfs:label>publishing house</rdfs:label>
      <skos:definition>Some business entity which specializes in publishing information.</skos:definition>
      <rdfs:subClassOf rdf:resource="&fibo-be-le-fbo;FormallyConstitutedOrganization"/>
   </owl:Class>


  <!--
    ///////////////////////////////////////////////////////////////////////////////////////
    //
    // Individuals
    //
    ///////////////////////////////////////////////////////////////////////////////////////
    -->


</rdf:RDF>