<?xml version="1.0" encoding="UTF-8"?>
  
<!DOCTYPE rdf:RDF [
    <!ENTITY fibo-fnd-pub-std "http://spec.edmcouncil.org/fibo/red/fnd/publications/standards/">
    <!ENTITY fibo-fnd-pub-pub "http://spec.edmcouncil.org/fibo/red/fnd/publications/publications/">
    <!ENTITY fibo-fnd-utl-bt "http://spec.edmcouncil.org/fibo/red/fnd/utilities/business-facing-types/">
    <!ENTITY fibo-be-le-fbo "http://spec.edmcouncil.org/fibo/red/be/legal-entities/formal-business-organizations/">
]>

<rdf:RDF xmlns:xsd="http://www.w3.org/2001/XMLSchema#"
         xmlns:sm="http://www.omg.org/techprocess/ab/SpecificationMetadata/"
         xmlns:xs="http://www.w3.org/2001/XMLSchema"
         xmlns:fibo-fnd-utl-av="http://www.omg.org/spec/EDMC-FIBO/FND/Utilities/AnnotationVocabulary/"
         xmlns:rdf="http://www.w3.org/1999/02/22-rdf-syntax-ns#"
         xmlns:rdfs="http://www.w3.org/2000/01/rdf-schema#"
         xmlns:owl="http://www.w3.org/2002/07/owl#"
         xmlns:skos="http://www.w3.org/2004/02/skos/core#"
         xmlns:dc="http://purl.org/dc/terms/"
         xml:base="http://spec.edmcouncil.org/fibo/red/fnd/publications/standards/">

   <owl:Ontology rdf:about="http://spec.edmcouncil.org/fibo/red/fnd/publications/standards/">
      <owl:imports rdf:resource="http://spec.edmcouncil.org/fibo/red/fnd/publications/publications/"/>
      <owl:imports rdf:resource="http://spec.edmcouncil.org/fibo/red/fnd/utilities/business-facing-types/"/>
      <owl:imports rdf:resource="http://spec.edmcouncil.org/fibo/red/be/legal-entities/formal-business-organizations/"/>
   </owl:Ontology>


  <!--
    ///////////////////////////////////////////////////////////////////////////////////////
    //
    // Datatypes
    //
    ///////////////////////////////////////////////////////////////////////////////////////
    -->



  <!--
    ///////////////////////////////////////////////////////////////////////////////////////
    //
    // Object Properties
    //
    ///////////////////////////////////////////////////////////////////////////////////////
    -->


<owl:ObjectProperty rdf:about="&fibo-fnd-pub-std;standardSetBy">
      <rdfs:label>standard set by</rdfs:label>
      <skos:definition>The agency by which the standard is set.</skos:definition>
      <rdfs:subPropertyOf rdf:resource="&fibo-fnd-pub-pub;publishedBy"/>
      <rdfs:domain rdf:resource="&fibo-fnd-pub-std;TechnicalStandard"/>
      <rdfs:range rdf:resource="&fibo-fnd-pub-std;StandardsSetter"/>
   </owl:ObjectProperty>

   <owl:ObjectProperty rdf:about="&fibo-fnd-pub-std;standardsSetterIdentity">
      <rdfs:label>standards setter identity</rdfs:label>
      <skos:definition>The entity which performs the role of Standards Setter.</skos:definition>
      <rdfs:subPropertyOf rdf:resource="&fibo-fnd-pub-pub;publisherIdentity"/>
      <rdfs:domain rdf:resource="&fibo-fnd-pub-std;StandardsSetter"/>
      <rdfs:range rdf:resource="&fibo-be-le-fbo;FormallyConstitutedOrganization"/>
   </owl:ObjectProperty>


  <!--
    ///////////////////////////////////////////////////////////////////////////////////////
    //
    // Data Properties
    //
    ///////////////////////////////////////////////////////////////////////////////////////
    -->


<owl:DatatypeProperty rdf:about="&fibo-fnd-pub-std;bodyAcronym">
      <rdfs:label>body acronym</rdfs:label>
      <skos:definition>The common acronym by which the standards body is referred in relation to the standards it sets e.g. FIX. Not necessarily the same as the legal name of the business entity that performs this role (e.g. FPL).</skos:definition>
      <rdfs:range rdf:resource="&fibo-fnd-utl-bt;text"/>
   </owl:DatatypeProperty>

   <owl:DatatypeProperty rdf:about="&fibo-fnd-pub-std;acronym">
      <rdfs:label>acronym</rdfs:label>
      <skos:definition>The abbreviation by which the Standard is referred.</skos:definition>
      <rdfs:range rdf:resource="&fibo-fnd-utl-bt;text"/>
   </owl:DatatypeProperty>

   <owl:DatatypeProperty rdf:about="&fibo-fnd-pub-std;standardName">
      <rdfs:label>standard name</rdfs:label>
      <skos:definition>The full formal name of the standard.</skos:definition>
      <rdfs:range rdf:resource="&fibo-fnd-utl-bt;text"/>
   </owl:DatatypeProperty>


  <!--
    ///////////////////////////////////////////////////////////////////////////////////////
    //
    // Annotation Properties
    //
    ///////////////////////////////////////////////////////////////////////////////////////
    -->



  <!--
    ///////////////////////////////////////////////////////////////////////////////////////
    //
    // Classes
    //
    ///////////////////////////////////////////////////////////////////////////////////////
    -->


<owl:Class rdf:about="&fibo-fnd-pub-std;IndustryAssociation">
      <rdfs:label>industry association</rdfs:label>
      <skos:definition>An organization which has membership drawn from members of some industry and acts to serve the interests of those members.</skos:definition>
      <rdfs:subClassOf rdf:resource="&fibo-be-le-fbo;FormallyConstitutedOrganization"/>
   </owl:Class>

   <owl:Class rdf:about="&fibo-fnd-pub-std;StandardsBody">
      <rdfs:label>standards body</rdfs:label>
      <skos:definition>An organization dedicated exclusively to the propagation of standards.</skos:definition>
   </owl:Class>

   <owl:Class rdf:about="&fibo-fnd-pub-std;StandardsSetter">
      <rdfs:label>standards setter</rdfs:label>
      <skos:definition>An agent which acts to set standards such as message standards, programming standards and so on. This may in principal be any kind of business entity.</skos:definition>
      <rdfs:subClassOf rdf:resource="&fibo-fnd-pub-pub;Publisher"/>
   </owl:Class>

   <owl:Class rdf:about="&fibo-fnd-pub-std;TechnicalStandard">
      <rdfs:label>technical standard</rdfs:label>
      <skos:definition>An established norm or requirement about technical systems; a published document formally setting out such established norm.</skos:definition>
      <rdfs:subClassOf rdf:resource="&fibo-fnd-pub-pub;PublishedInformation"/>
   </owl:Class>


  <!--
    ///////////////////////////////////////////////////////////////////////////////////////
    //
    // Individuals
    //
    ///////////////////////////////////////////////////////////////////////////////////////
    -->


</rdf:RDF>