<?xml version="1.0" encoding="UTF-8"?>
<!DOCTYPE rdf:RDF [
	<!ENTITY dct "http://purl.org/dc/terms/">
	<!ENTITY fibo-be-le-fbo "https://spec.edmcouncil.org/fibo/ontology/BE/LegalEntities/FormalBusinessOrganizations/">
	<!ENTITY fibo-be-oac-exec "https://spec.edmcouncil.org/fibo/ontology/BE/OwnershipAndControl/Executives/">
	<!ENTITY fibo-fbc-dae-dbt "https://spec.edmcouncil.org/fibo/ontology/FBC/DebtAndEquities/Debt/">
	<!ENTITY fibo-fbc-fct-fse "https://spec.edmcouncil.org/fibo/ontology/FBC/FunctionalEntities/FinancialServicesEntities/">
	<!ENTITY fibo-fbc-fi-fi "https://spec.edmcouncil.org/fibo/ontology/FBC/FinancialInstruments/FinancialInstruments/">
	<!ENTITY fibo-fbc-pas-caa "https://spec.edmcouncil.org/fibo/ontology/FBC/ProductsAndServices/ClientsAndAccounts/">
	<!ENTITY fibo-fbc-pas-fpas "https://spec.edmcouncil.org/fibo/ontology/FBC/ProductsAndServices/FinancialProductsAndServices/">
	<!ENTITY fibo-fnd-aap-agt "https://spec.edmcouncil.org/fibo/ontology/FND/AgentsAndPeople/Agents/">
	<!ENTITY fibo-fnd-acc-cur "https://spec.edmcouncil.org/fibo/ontology/FND/Accounting/CurrencyAmount/">
	<!ENTITY fibo-fnd-agr-ctr "https://spec.edmcouncil.org/fibo/ontology/FND/Agreements/Contracts/">
	<!ENTITY fibo-fnd-arr-arr "https://spec.edmcouncil.org/fibo/ontology/FND/Arrangements/Arrangements/">
	<!ENTITY fibo-fnd-arr-doc "https://spec.edmcouncil.org/fibo/ontology/FND/Arrangements/Documents/">
	<!ENTITY fibo-fnd-arr-id "https://spec.edmcouncil.org/fibo/ontology/FND/Arrangements/IdentifiersAndIndices/">
	<!ENTITY fibo-fnd-dt-fd "https://spec.edmcouncil.org/fibo/ontology/FND/DatesAndTimes/FinancialDates/">
	<!ENTITY fibo-fnd-oac-own "https://spec.edmcouncil.org/fibo/ontology/FND/OwnershipAndControl/Ownership/">
	<!ENTITY fibo-fnd-pas-pas "https://spec.edmcouncil.org/fibo/ontology/FND/ProductsAndServices/ProductsAndServices/">
	<!ENTITY fibo-fnd-pty-pty "https://spec.edmcouncil.org/fibo/ontology/FND/Parties/Parties/">
	<!ENTITY fibo-fnd-pty-rl "https://spec.edmcouncil.org/fibo/ontology/FND/Parties/Roles/">
	<!ENTITY fibo-fnd-rel-rel "https://spec.edmcouncil.org/fibo/ontology/FND/Relations/Relations/">
	<!ENTITY fibo-fnd-utl-av "https://spec.edmcouncil.org/fibo/ontology/FND/Utilities/AnnotationVocabulary/">
	<!ENTITY lcc-cr "https://www.omg.org/spec/LCC/Countries/CountryRepresentation/">
	<!ENTITY owl "http://www.w3.org/2002/07/owl#">
	<!ENTITY rdf "http://www.w3.org/1999/02/22-rdf-syntax-ns#">
	<!ENTITY rdfs "http://www.w3.org/2000/01/rdf-schema#">
	<!ENTITY skos "http://www.w3.org/2004/02/skos/core#">
	<!ENTITY sm "http://www.omg.org/techprocess/ab/SpecificationMetadata/">
	<!ENTITY xsd "http://www.w3.org/2001/XMLSchema#">
]>
<rdf:RDF xml:base="https://spec.edmcouncil.org/fibo/ontology/FBC/ProductsAndServices/ClientsAndAccounts/"
	xmlns:dct="http://purl.org/dc/terms/"
	xmlns:fibo-be-le-fbo="https://spec.edmcouncil.org/fibo/ontology/BE/LegalEntities/FormalBusinessOrganizations/"
	xmlns:fibo-be-oac-exec="https://spec.edmcouncil.org/fibo/ontology/BE/OwnershipAndControl/Executives/"
	xmlns:fibo-fbc-dae-dbt="https://spec.edmcouncil.org/fibo/ontology/FBC/DebtAndEquities/Debt/"
	xmlns:fibo-fbc-fct-fse="https://spec.edmcouncil.org/fibo/ontology/FBC/FunctionalEntities/FinancialServicesEntities/"
	xmlns:fibo-fbc-fi-fi="https://spec.edmcouncil.org/fibo/ontology/FBC/FinancialInstruments/FinancialInstruments/"
	xmlns:fibo-fbc-pas-caa="https://spec.edmcouncil.org/fibo/ontology/FBC/ProductsAndServices/ClientsAndAccounts/"
	xmlns:fibo-fbc-pas-fpas="https://spec.edmcouncil.org/fibo/ontology/FBC/ProductsAndServices/FinancialProductsAndServices/"
	xmlns:fibo-fnd-aap-agt="https://spec.edmcouncil.org/fibo/ontology/FND/AgentsAndPeople/Agents/"
	xmlns:fibo-fnd-acc-cur="https://spec.edmcouncil.org/fibo/ontology/FND/Accounting/CurrencyAmount/"
	xmlns:fibo-fnd-agr-ctr="https://spec.edmcouncil.org/fibo/ontology/FND/Agreements/Contracts/"
	xmlns:fibo-fnd-arr-arr="https://spec.edmcouncil.org/fibo/ontology/FND/Arrangements/Arrangements/"
	xmlns:fibo-fnd-arr-doc="https://spec.edmcouncil.org/fibo/ontology/FND/Arrangements/Documents/"
	xmlns:fibo-fnd-arr-id="https://spec.edmcouncil.org/fibo/ontology/FND/Arrangements/IdentifiersAndIndices/"
	xmlns:fibo-fnd-dt-fd="https://spec.edmcouncil.org/fibo/ontology/FND/DatesAndTimes/FinancialDates/"
	xmlns:fibo-fnd-oac-own="https://spec.edmcouncil.org/fibo/ontology/FND/OwnershipAndControl/Ownership/"
	xmlns:fibo-fnd-pas-pas="https://spec.edmcouncil.org/fibo/ontology/FND/ProductsAndServices/ProductsAndServices/"
	xmlns:fibo-fnd-pty-pty="https://spec.edmcouncil.org/fibo/ontology/FND/Parties/Parties/"
	xmlns:fibo-fnd-pty-rl="https://spec.edmcouncil.org/fibo/ontology/FND/Parties/Roles/"
	xmlns:fibo-fnd-rel-rel="https://spec.edmcouncil.org/fibo/ontology/FND/Relations/Relations/"
	xmlns:fibo-fnd-utl-av="https://spec.edmcouncil.org/fibo/ontology/FND/Utilities/AnnotationVocabulary/"
	xmlns:lcc-cr="https://www.omg.org/spec/LCC/Countries/CountryRepresentation/"
	xmlns:owl="http://www.w3.org/2002/07/owl#"
	xmlns:rdf="http://www.w3.org/1999/02/22-rdf-syntax-ns#"
	xmlns:rdfs="http://www.w3.org/2000/01/rdf-schema#"
	xmlns:skos="http://www.w3.org/2004/02/skos/core#"
	xmlns:sm="http://www.omg.org/techprocess/ab/SpecificationMetadata/"
	xmlns:xsd="http://www.w3.org/2001/XMLSchema#">
	
	<owl:Ontology rdf:about="https://spec.edmcouncil.org/fibo/ontology/FBC/ProductsAndServices/ClientsAndAccounts/">
		<rdfs:label>Clients and Accounts Ontology</rdfs:label>
		<dct:abstract>This ontology provides basic concepts such as account, account holder, account provider, relationship manager that are commonly used by financial services providers to describe customers and to determine counterparty identities.</dct:abstract>
		<dct:license rdf:datatype="&xsd;anyURI">http://opensource.org/licenses/MIT</dct:license>
		<sm:contentLanguage rdf:datatype="&xsd;anyURI">http://www.w3.org/standards/techs/owl#w3c_all</sm:contentLanguage>
		<sm:copyright>Copyright (c) 2015-2020 EDM Council, Inc.</sm:copyright>
		<sm:copyright>Copyright (c) 2015-2020 Object Management Group, Inc.</sm:copyright>
		<sm:dependsOn rdf:resource="https://spec.edmcouncil.org/fibo/ontology/BE/"/>
		<sm:dependsOn rdf:resource="https://spec.edmcouncil.org/fibo/ontology/FBC/ProductsAndServices/FinancialProductsAndServices/"/>
		<sm:dependsOn rdf:resource="https://spec.edmcouncil.org/fibo/ontology/FND/"/>
		<sm:fileAbbreviation>fibo-fbc-pas-caa</sm:fileAbbreviation>
		<sm:filename>ClientsAndAccounts.rdf</sm:filename>
		<owl:imports rdf:resource="https://spec.edmcouncil.org/fibo/ontology/BE/LegalEntities/FormalBusinessOrganizations/"/>
		<owl:imports rdf:resource="https://spec.edmcouncil.org/fibo/ontology/BE/OwnershipAndControl/Executives/"/>
		<owl:imports rdf:resource="https://spec.edmcouncil.org/fibo/ontology/FBC/DebtAndEquities/Debt/"/>
		<owl:imports rdf:resource="https://spec.edmcouncil.org/fibo/ontology/FBC/FinancialInstruments/FinancialInstruments/"/>
		<owl:imports rdf:resource="https://spec.edmcouncil.org/fibo/ontology/FBC/FunctionalEntities/FinancialServicesEntities/"/>
		<owl:imports rdf:resource="https://spec.edmcouncil.org/fibo/ontology/FBC/ProductsAndServices/FinancialProductsAndServices/"/>
		<owl:imports rdf:resource="https://spec.edmcouncil.org/fibo/ontology/FND/Accounting/CurrencyAmount/"/>
		<owl:imports rdf:resource="https://spec.edmcouncil.org/fibo/ontology/FND/AgentsAndPeople/Agents/"/>
		<owl:imports rdf:resource="https://spec.edmcouncil.org/fibo/ontology/FND/Agreements/Contracts/"/>
		<owl:imports rdf:resource="https://spec.edmcouncil.org/fibo/ontology/FND/Arrangements/Arrangements/"/>
		<owl:imports rdf:resource="https://spec.edmcouncil.org/fibo/ontology/FND/Arrangements/Documents/"/>
		<owl:imports rdf:resource="https://spec.edmcouncil.org/fibo/ontology/FND/Arrangements/IdentifiersAndIndices/"/>
		<owl:imports rdf:resource="https://spec.edmcouncil.org/fibo/ontology/FND/DatesAndTimes/FinancialDates/"/>
		<owl:imports rdf:resource="https://spec.edmcouncil.org/fibo/ontology/FND/DatesAndTimes/Occurrences/"/>
		<owl:imports rdf:resource="https://spec.edmcouncil.org/fibo/ontology/FND/OwnershipAndControl/Ownership/"/>
		<owl:imports rdf:resource="https://spec.edmcouncil.org/fibo/ontology/FND/Parties/Parties/"/>
		<owl:imports rdf:resource="https://spec.edmcouncil.org/fibo/ontology/FND/Parties/Roles/"/>
		<owl:imports rdf:resource="https://spec.edmcouncil.org/fibo/ontology/FND/ProductsAndServices/ProductsAndServices/"/>
		<owl:imports rdf:resource="https://spec.edmcouncil.org/fibo/ontology/FND/Relations/Relations/"/>
		<owl:imports rdf:resource="https://spec.edmcouncil.org/fibo/ontology/FND/Utilities/AnnotationVocabulary/"/>
		<owl:imports rdf:resource="https://www.omg.org/spec/LCC/Countries/CountryRepresentation/"/>
		<owl:versionIRI rdf:resource="https://spec.edmcouncil.org/fibo/ontology/FBC/20200101/ProductsAndServices/ClientsAndAccounts/"/>
		<skos:changeNote>The https://spec.edmcouncil.org/fibo/ontology/FBC/20160801/ProductsAndServices/ClientsAndAccounts.rdf version of this ontology was revised per the FIBO 2.0 RFC with respect to the definitions for accounts and account identifiers, such as BBAN and IBAN identifiers, including but not limited to bank accounts.</skos:changeNote>
		<skos:changeNote>The https://spec.edmcouncil.org/fibo/ontology/FBC/20180801/ProductsAndServices/ClientsAndAccounts/ version of this ontology was modified to support the addition of maturity-related properties to financial instruments.</skos:changeNote>
		<skos:changeNote>The https://spec.edmcouncil.org/fibo/ontology/FBC/20181101/ProductsAndServices/ClientsAndAccounts/ version of this ontology was modified to replace hasDefinition with isDefinedIn to clarify intent.</skos:changeNote>
		<skos:changeNote>The https://spec.edmcouncil.org/fibo/ontology/FBC/20190701/ProductsAndServices/ClientsAndAccounts.rdf version of this ontology was revised to eliminate deprecated elements.</skos:changeNote>
		<skos:changeNote>The https://spec.edmcouncil.org/fibo/ontology/FBC/20190901/ProductsAndServices/ClientsAndAccounts.rdf version of this ontology was revised to eliminate the disjointness between a deposit account and investment account to allow for certain portfolio management accounts that have characteristics of both.</skos:changeNote>
		<skos:changeNote>The https://spec.edmcouncil.org/fibo/ontology/FBC/20191201/ProductsAndServices/ClientsAndAccounts.rdf version of this ontology was revised to add definitions for balance, fee, general ledger, ledger account, income and related properties, and revise definitions to be ISO 704 compliant.</skos:changeNote>
		<fibo-fnd-utl-av:hasMaturityLevel rdf:resource="&fibo-fnd-utl-av;Release"/>
	</owl:Ontology>
	
	<owl:Class rdf:about="&fibo-fbc-pas-caa;Account">
		<rdfs:subClassOf>
			<owl:Restriction>
				<owl:onProperty rdf:resource="&fibo-fnd-aap-agt;isIdentifiedBy"/>
				<owl:onClass rdf:resource="&fibo-fbc-pas-caa;AccountIdentifier"/>
				<owl:minQualifiedCardinality rdf:datatype="&xsd;nonNegativeInteger">0</owl:minQualifiedCardinality>
			</owl:Restriction>
		</rdfs:subClassOf>
		<rdfs:subClassOf>
			<owl:Restriction>
				<owl:onProperty rdf:resource="&fibo-fnd-rel-rel;comprises"/>
				<owl:onClass rdf:resource="&fibo-fnd-arr-doc;Record"/>
				<owl:minQualifiedCardinality rdf:datatype="&xsd;nonNegativeInteger">0</owl:minQualifiedCardinality>
			</owl:Restriction>
		</rdfs:subClassOf>
		<rdfs:subClassOf>
			<owl:Restriction>
				<owl:onProperty rdf:resource="&fibo-fbc-pas-caa;hasAccountCloseDate"/>
				<owl:onClass rdf:resource="&fibo-fnd-dt-fd;ExplicitDate"/>
				<owl:minQualifiedCardinality rdf:datatype="&xsd;nonNegativeInteger">0</owl:minQualifiedCardinality>
			</owl:Restriction>
		</rdfs:subClassOf>
		<rdfs:subClassOf>
			<owl:Restriction>
				<owl:onProperty rdf:resource="&fibo-fbc-pas-caa;hasAccountOpenDate"/>
				<owl:onClass rdf:resource="&fibo-fnd-dt-fd;ExplicitDate"/>
				<owl:qualifiedCardinality rdf:datatype="&xsd;nonNegativeInteger">1</owl:qualifiedCardinality>
			</owl:Restriction>
		</rdfs:subClassOf>
		<rdfs:subClassOf>
			<owl:Restriction>
				<owl:onProperty rdf:resource="&fibo-fbc-pas-caa;hasBalance"/>
				<owl:someValuesFrom rdf:resource="&fibo-fbc-pas-caa;Balance"/>
			</owl:Restriction>
		</rdfs:subClassOf>
		<rdfs:subClassOf>
			<owl:Restriction>
				<owl:onProperty rdf:resource="&fibo-fnd-rel-rel;isProvidedBy"/>
				<owl:someValuesFrom rdf:resource="&fibo-fbc-pas-caa;AccountProvider"/>
			</owl:Restriction>
		</rdfs:subClassOf>
		<rdfs:label>account</rdfs:label>
		<skos:definition>container for records associated with a business arrangement for regular dealings or services (such as personal or professional services, banking)</skos:definition>
		<fibo-fnd-utl-av:explanatoryNote>In general, an account is associated with a contractual relationship between a buyer and seller under which payment may be made at a later time.</fibo-fnd-utl-av:explanatoryNote>
	</owl:Class>
	
	<owl:Class rdf:about="&fibo-fbc-pas-caa;AccountHolder">
		<rdfs:subClassOf rdf:resource="&fibo-fnd-oac-own;Owner"/>
		<rdfs:subClassOf>
			<owl:Restriction>
				<owl:onProperty rdf:resource="&fibo-fnd-pty-rl;isPlayedBy"/>
				<owl:someValuesFrom>
					<owl:Restriction>
						<owl:onProperty rdf:resource="&fibo-fnd-oac-own;owns"/>
						<owl:someValuesFrom rdf:resource="&fibo-fbc-pas-caa;Account"/>
					</owl:Restriction>
				</owl:someValuesFrom>
			</owl:Restriction>
		</rdfs:subClassOf>
		<rdfs:subClassOf>
			<owl:Restriction>
				<owl:onProperty rdf:resource="&fibo-fnd-pty-rl;isPlayedBy"/>
				<owl:someValuesFrom>
					<owl:Restriction>
						<owl:onProperty rdf:resource="&fibo-fnd-pty-pty;isAPartyTo"/>
						<owl:someValuesFrom rdf:resource="&fibo-fbc-pas-caa;Account"/>
					</owl:Restriction>
				</owl:someValuesFrom>
			</owl:Restriction>
		</rdfs:subClassOf>
		<rdfs:label>account holder</rdfs:label>
		<skos:definition>party holding an account</skos:definition>
	</owl:Class>
	
	<owl:Class rdf:about="&fibo-fbc-pas-caa;AccountIdentifier">
		<rdfs:subClassOf rdf:resource="&fibo-fnd-arr-id;Identifier"/>
		<rdfs:subClassOf>
			<owl:Restriction>
				<owl:onProperty rdf:resource="&fibo-fnd-aap-agt;identifies"/>
				<owl:onClass rdf:resource="&fibo-fbc-pas-caa;Account"/>
				<owl:qualifiedCardinality rdf:datatype="&xsd;nonNegativeInteger">1</owl:qualifiedCardinality>
			</owl:Restriction>
		</rdfs:subClassOf>
		<rdfs:label>account identifier</rdfs:label>
		<skos:definition>identifier that denotes an account</skos:definition>
		<fibo-fnd-utl-av:adaptedFrom>ISO 13616-1:2007 Financial services - International bank account number (IBAN)</fibo-fnd-utl-av:adaptedFrom>
		<fibo-fnd-utl-av:synonym>account number</fibo-fnd-utl-av:synonym>
	</owl:Class>
	
	<owl:Class rdf:about="&fibo-fbc-pas-caa;AccountProvider">
		<rdfs:subClassOf rdf:resource="&fibo-fnd-pas-pas;ServiceProvider"/>
		<rdfs:subClassOf>
			<owl:Restriction>
				<owl:onProperty rdf:resource="&fibo-fnd-pty-rl;isPlayedBy"/>
				<owl:someValuesFrom>
					<owl:Restriction>
						<owl:onProperty rdf:resource="&fibo-fnd-pty-pty;isAPartyTo"/>
						<owl:someValuesFrom rdf:resource="&fibo-fbc-pas-caa;Account"/>
					</owl:Restriction>
				</owl:someValuesFrom>
			</owl:Restriction>
		</rdfs:subClassOf>
		<rdfs:label>account provider</rdfs:label>
		<skos:definition>party that provides and services the account</skos:definition>
	</owl:Class>
	
	<owl:Class rdf:about="&fibo-fbc-pas-caa;AccountSpecificServiceAgreement">
		<rdfs:subClassOf rdf:resource="&fibo-fnd-pas-pas;ServiceAgreement"/>
		<rdfs:subClassOf>
			<owl:Restriction>
				<owl:onProperty rdf:resource="&fibo-fnd-agr-ctr;hasContractParty"/>
				<owl:someValuesFrom rdf:resource="&fibo-fbc-pas-caa;AccountHolder"/>
			</owl:Restriction>
		</rdfs:subClassOf>
		<rdfs:subClassOf>
			<owl:Restriction>
				<owl:onProperty rdf:resource="&fibo-fnd-agr-ctr;hasContractParty"/>
				<owl:someValuesFrom rdf:resource="&fibo-fbc-pas-caa;AccountProvider"/>
			</owl:Restriction>
		</rdfs:subClassOf>
		<rdfs:subClassOf>
			<owl:Restriction>
				<owl:onProperty rdf:resource="&fibo-fnd-rel-rel;appliesTo"/>
				<owl:someValuesFrom rdf:resource="&fibo-fbc-pas-caa;Account"/>
			</owl:Restriction>
		</rdfs:subClassOf>
		<rdfs:label>account-specific service agreement</rdfs:label>
		<skos:definition>service-agreement that is account-specific, applicable in cases where a client holds multiple accounts with differing terms and conditions</skos:definition>
		<fibo-fnd-utl-av:explanatoryNote>Customers of financial service providers frequently hold multiple accounts - brokerage accounts, checking and savings accounts, trust accounts, and so forth - which may have specific terms and conditions associated with them.</fibo-fnd-utl-av:explanatoryNote>
	</owl:Class>
	
	<owl:Class rdf:about="&fibo-fbc-pas-caa;AccountingTransaction">
		<rdfs:subClassOf rdf:resource="&fibo-fnd-pas-pas;TransactionEvent"/>
		<rdfs:label>accounting transaction</rdfs:label>
		<skos:definition>event or condition recognized by an entry in the records of an account</skos:definition>
	</owl:Class>
	
	<owl:Class rdf:about="&fibo-fbc-pas-caa;Balance">
		<rdfs:subClassOf rdf:resource="&fibo-fnd-acc-cur;MonetaryAmount"/>
		<rdfs:label>balance</rdfs:label>
		<skos:definition>amount of money available or owed</skos:definition>
		<fibo-fnd-utl-av:explanatoryNote>The balance is the net amount after factoring in all debits and credits, including service charges and fees.</fibo-fnd-utl-av:explanatoryNote>
	</owl:Class>
	
	<owl:Class rdf:about="&fibo-fbc-pas-caa;BankAccount">
		<rdfs:subClassOf rdf:resource="&fibo-fbc-pas-caa;Account"/>
		<rdfs:subClassOf>
			<owl:Restriction>
				<owl:onProperty rdf:resource="&fibo-fnd-aap-agt;isIdentifiedBy"/>
				<owl:someValuesFrom rdf:resource="&fibo-fbc-pas-caa;BankAccountIdentifier"/>
			</owl:Restriction>
		</rdfs:subClassOf>
		<rdfs:subClassOf>
			<owl:Restriction>
				<owl:onProperty rdf:resource="&fibo-fnd-rel-rel;isProvidedBy"/>
				<owl:someValuesFrom rdf:resource="&fibo-fbc-fct-fse;Bank"/>
			</owl:Restriction>
		</rdfs:subClassOf>
		<rdfs:label>bank account</rdfs:label>
		<skos:definition>account held or provided by, as a service, a bank</skos:definition>
	</owl:Class>
	
	<owl:Class rdf:about="&fibo-fbc-pas-caa;BankAccountIdentifier">
		<rdfs:subClassOf rdf:resource="&fibo-fbc-pas-caa;AccountIdentifier"/>
		<rdfs:subClassOf>
			<owl:Restriction>
				<owl:onProperty rdf:resource="&fibo-fnd-aap-agt;identifies"/>
				<owl:onClass rdf:resource="&fibo-fbc-pas-caa;BankAccount"/>
				<owl:qualifiedCardinality rdf:datatype="&xsd;nonNegativeInteger">1</owl:qualifiedCardinality>
			</owl:Restriction>
		</rdfs:subClassOf>
		<rdfs:label>bank account identifier</rdfs:label>
		<skos:definition>identifier that identifies a bank account</skos:definition>
		<fibo-fnd-utl-av:adaptedFrom>ISO 13616-1:2007 Financial services - International bank account number (IBAN)</fibo-fnd-utl-av:adaptedFrom>
		<fibo-fnd-utl-av:synonym>bank account number</fibo-fnd-utl-av:synonym>
	</owl:Class>
	
	<owl:Class rdf:about="&fibo-fbc-pas-caa;BankIdentifier">
		<rdfs:subClassOf rdf:resource="&fibo-be-le-fbo;OrganizationIdentifier"/>
		<rdfs:subClassOf>
			<owl:Restriction>
				<owl:onProperty rdf:resource="&fibo-fnd-aap-agt;identifies"/>
				<owl:onClass rdf:resource="&fibo-fbc-fct-fse;Bank"/>
				<owl:qualifiedCardinality rdf:datatype="&xsd;nonNegativeInteger">1</owl:qualifiedCardinality>
			</owl:Restriction>
		</rdfs:subClassOf>
		<rdfs:label>bank identifier</rdfs:label>
		<skos:definition>identifier that uniquely identifies the financial institution and, when appropriate, the branch of that financial institution servicing an account</skos:definition>
		<fibo-fnd-utl-av:adaptedFrom>ISO 13616-1:2007 Financial services - International bank account number (IBAN)</fibo-fnd-utl-av:adaptedFrom>
		<fibo-fnd-utl-av:synonym>bank number</fibo-fnd-utl-av:synonym>
	</owl:Class>
	
	<owl:Class rdf:about="&fibo-fbc-pas-caa;BasicBankAccountIdentifier">
		<rdfs:subClassOf rdf:resource="&fibo-fbc-pas-caa;BankAccountIdentifier"/>
		<rdfs:subClassOf>
			<owl:Restriction>
				<owl:onProperty rdf:resource="&fibo-fnd-rel-rel;comprises"/>
				<owl:onClass rdf:resource="&fibo-fbc-pas-caa;BankAccountIdentifier"/>
				<owl:qualifiedCardinality rdf:datatype="&xsd;nonNegativeInteger">1</owl:qualifiedCardinality>
			</owl:Restriction>
		</rdfs:subClassOf>
		<rdfs:subClassOf>
			<owl:Restriction>
				<owl:onProperty rdf:resource="&fibo-fnd-rel-rel;comprises"/>
				<owl:onClass rdf:resource="&fibo-fbc-pas-caa;BankIdentifier"/>
				<owl:qualifiedCardinality rdf:datatype="&xsd;nonNegativeInteger">1</owl:qualifiedCardinality>
			</owl:Restriction>
		</rdfs:subClassOf>
		<rdfs:label>basic bank account identifier</rdfs:label>
		<skos:definition>identifier that uniquely identifies an individual account at a specific financial institution in a particular country and which includes a bank identifier of the financial institution servicing that account</skos:definition>
		<fibo-fnd-utl-av:abbreviation>BBAN</fibo-fnd-utl-av:abbreviation>
		<fibo-fnd-utl-av:adaptedFrom>ISO 13616-1:2007 Financial services - International bank account number (IBAN)</fibo-fnd-utl-av:adaptedFrom>
		<fibo-fnd-utl-av:synonym>basic bank account number</fibo-fnd-utl-av:synonym>
	</owl:Class>
	
	<owl:Class rdf:about="&fibo-fbc-pas-caa;BrokerageAccount">
		<rdfs:subClassOf rdf:resource="&fibo-fbc-pas-caa;InvestmentAccount"/>
		<rdfs:subClassOf>
			<owl:Restriction>
				<owl:onProperty rdf:resource="&fibo-fnd-rel-rel;isProvidedBy"/>
				<owl:someValuesFrom>
					<owl:Class>
						<owl:unionOf rdf:parseType="Collection">
							<rdf:Description rdf:about="&fibo-fbc-fct-fse;Bank">
							</rdf:Description>
							<rdf:Description rdf:about="&fibo-fbc-fct-fse;BrokerageFirm">
							</rdf:Description>
							<rdf:Description rdf:about="&fibo-fbc-fct-fse;FuturesCommissionMerchant">
							</rdf:Description>
						</owl:unionOf>
					</owl:Class>
				</owl:someValuesFrom>
			</owl:Restriction>
		</rdfs:subClassOf>
		<rdfs:label>brokerage account</rdfs:label>
		<skos:definition>account offered by a broker that allows the investor to deposit funds and place investment orders</skos:definition>
		<fibo-fnd-utl-av:explanatoryNote>The investor owns the assets contained in the brokerage account and must usually claim as income any capital gains incurred.</fibo-fnd-utl-av:explanatoryNote>
	</owl:Class>
	
	<owl:Class rdf:about="&fibo-fbc-pas-caa;CertificateOfDeposit">
		<rdfs:subClassOf rdf:resource="&fibo-fbc-fi-fi;CashInstrument"/>
		<rdfs:subClassOf>
			<owl:Restriction>
				<owl:onProperty rdf:resource="&fibo-fbc-dae-dbt;hasInterestRate"/>
				<owl:onClass rdf:resource="&fibo-fnd-acc-cur;InterestRate"/>
				<owl:qualifiedCardinality rdf:datatype="&xsd;nonNegativeInteger">1</owl:qualifiedCardinality>
			</owl:Restriction>
		</rdfs:subClassOf>
		<rdfs:subClassOf>
			<owl:Restriction>
				<owl:onProperty rdf:resource="&fibo-fnd-acc-cur;hasNotionalAmount"/>
				<owl:onClass rdf:resource="&fibo-fnd-acc-cur;MonetaryAmount"/>
				<owl:qualifiedCardinality rdf:datatype="&xsd;nonNegativeInteger">1</owl:qualifiedCardinality>
			</owl:Restriction>
		</rdfs:subClassOf>
		<rdfs:subClassOf>
			<owl:Restriction>
				<owl:onProperty rdf:resource="&fibo-fbc-fi-fi;hasTerm"/>
				<owl:onClass rdf:resource="&fibo-fnd-dt-fd;Duration"/>
				<owl:qualifiedCardinality rdf:datatype="&xsd;nonNegativeInteger">1</owl:qualifiedCardinality>
			</owl:Restriction>
		</rdfs:subClassOf>
		<rdfs:label xml:lang="en">certificate of deposit</rdfs:label>
		<skos:definition xml:lang="en">cash instrument associated with a time deposit account that cannot be withdrawn for a certain &quot;term&quot; or period of time.</skos:definition>
		<fibo-fnd-utl-av:abbreviation>CD</fibo-fnd-utl-av:abbreviation>
		<fibo-fnd-utl-av:explanatoryNote>When the term is over it can be withdrawn or it can be held for another term. The longer the term the better the yield on the money.</fibo-fnd-utl-av:explanatoryNote>
	</owl:Class>
	
	<owl:Class rdf:about="&fibo-fbc-pas-caa;DemandDepositAccount">
		<rdfs:subClassOf rdf:resource="&fibo-fbc-pas-caa;TransactionDepositAccount"/>
		<rdfs:label>demand deposit account</rdfs:label>
		<skos:definition>non-interest-bearing deposit account in which deposits are payable immediately on demand, or that are issued with an original maturity or required notice period of less than seven days, or that represent funds for which the depository institution does not reserve the right to require at least seven days&apos; written notice of an intended withdrawal</skos:definition>
		<fibo-fnd-utl-av:abbreviation>DDA</fibo-fnd-utl-av:abbreviation>
		<fibo-fnd-utl-av:adaptedFrom>https://www.fdic.gov/regulations/resources/call/crinst/2010-09/910gloss_093010.pdf</fibo-fnd-utl-av:adaptedFrom>
		<fibo-fnd-utl-av:explanatoryNote>Demand deposits include any matured time deposits without automatic renewal provisions, unless the deposit agreement provides for the funds to be transferred at maturity to another type of account. Demand deposits do not include: (i) money market deposit accounts (MMDAs) or (ii) NOW accounts.</fibo-fnd-utl-av:explanatoryNote>
	</owl:Class>
	
	<owl:Class rdf:about="&fibo-fbc-pas-caa;DepositAccount">
		<rdfs:subClassOf rdf:resource="&fibo-fbc-fct-fse;BankingProduct"/>
		<rdfs:subClassOf rdf:resource="&fibo-fbc-pas-caa;InvestmentOrDepositAccount"/>
		<rdfs:subClassOf>
			<owl:Restriction>
				<owl:onProperty rdf:resource="&fibo-fnd-rel-rel;isProvidedBy"/>
				<owl:someValuesFrom rdf:resource="&fibo-fbc-fct-fse;DepositoryInstitution"/>
			</owl:Restriction>
		</rdfs:subClassOf>
		<rdfs:label>deposit account</rdfs:label>
		<skos:definition>account that provides a record of money placed with a depository institution for safekeeping and management</skos:definition>
		<skos:example>Deposit accounts include savings accounts, money market accounts, and transactional accounts, such as demand deposit accounts, among others.</skos:example>
		<fibo-fnd-utl-av:explanatoryNote>The account holder has the right to withdraw deposited funds, as set forth in the terms and conditions governing the account agreement. Deposit accounts may be insured up to a certain amount, depending on the jurisdiction.</fibo-fnd-utl-av:explanatoryNote>
	</owl:Class>
	
	<owl:Class rdf:about="&fibo-fbc-pas-caa;Fee">
		<rdfs:subClassOf rdf:resource="&fibo-fnd-acc-cur;MonetaryAmount"/>
		<rdfs:label>fee</rdfs:label>
		<skos:definition>charge for services performed</skos:definition>
	</owl:Class>
	
	<owl:Class rdf:about="&fibo-fbc-pas-caa;FinancialServiceAccount">
		<rdfs:subClassOf rdf:resource="&fibo-fbc-pas-caa;Account"/>
		<rdfs:subClassOf>
			<owl:Restriction>
				<owl:onProperty rdf:resource="&fibo-fbc-pas-caa;realizes"/>
				<owl:someValuesFrom>
					<owl:Class>
						<owl:unionOf rdf:parseType="Collection">
							<rdf:Description rdf:about="&fibo-fbc-pas-fpas;FinancialProduct">
							</rdf:Description>
							<rdf:Description rdf:about="&fibo-fbc-pas-fpas;FinancialService">
							</rdf:Description>
						</owl:unionOf>
					</owl:Class>
				</owl:someValuesFrom>
			</owl:Restriction>
		</rdfs:subClassOf>
		<rdfs:subClassOf>
			<owl:Restriction>
				<owl:onProperty rdf:resource="&fibo-fnd-aap-agt;isIdentifiedBy"/>
				<owl:someValuesFrom rdf:resource="&fibo-fbc-pas-caa;AccountIdentifier"/>
			</owl:Restriction>
		</rdfs:subClassOf>
		<rdfs:subClassOf>
			<owl:Restriction>
				<owl:onProperty rdf:resource="&fibo-fnd-pty-pty;hasPartyInRole"/>
				<owl:someValuesFrom>
					<owl:Class>
						<owl:intersectionOf rdf:parseType="Collection">
							<rdf:Description rdf:about="&fibo-fbc-pas-caa;AccountHolder">
							</rdf:Description>
							<owl:Class>
								<owl:unionOf rdf:parseType="Collection">
									<rdf:Description rdf:about="&fibo-fnd-pas-pas;Client">
									</rdf:Description>
									<rdf:Description rdf:about="&fibo-fnd-pas-pas;Customer">
									</rdf:Description>
								</owl:unionOf>
							</owl:Class>
						</owl:intersectionOf>
					</owl:Class>
				</owl:someValuesFrom>
			</owl:Restriction>
		</rdfs:subClassOf>
		<rdfs:subClassOf>
			<owl:Restriction>
				<owl:onProperty rdf:resource="&fibo-fnd-rel-rel;isDefinedIn"/>
				<owl:someValuesFrom rdf:resource="&fibo-fnd-pas-pas;ServiceAgreement"/>
			</owl:Restriction>
		</rdfs:subClassOf>
		<rdfs:subClassOf>
			<owl:Restriction>
				<owl:onProperty rdf:resource="&fibo-fnd-rel-rel;isProvidedBy"/>
				<owl:someValuesFrom>
					<owl:Class>
						<owl:intersectionOf rdf:parseType="Collection">
							<rdf:Description rdf:about="&fibo-fbc-pas-caa;AccountProvider">
							</rdf:Description>
							<rdf:Description rdf:about="&fibo-fbc-pas-fpas;FinancialServiceProvider">
							</rdf:Description>
						</owl:intersectionOf>
					</owl:Class>
				</owl:someValuesFrom>
			</owl:Restriction>
		</rdfs:subClassOf>
		<rdfs:label>financial service account</rdfs:label>
		<skos:definition>account provided by a financial service provider associated with a specific financial product or service</skos:definition>
	</owl:Class>
	
	<owl:Class rdf:about="&fibo-fbc-pas-caa;GeneralLedger">
		<rdfs:subClassOf rdf:resource="&fibo-fnd-arr-doc;Record"/>
		<rdfs:subClassOf>
			<owl:Restriction>
				<owl:onProperty rdf:resource="&fibo-fnd-rel-rel;comprises"/>
				<owl:someValuesFrom rdf:resource="&fibo-fbc-pas-caa;LedgerAccount"/>
			</owl:Restriction>
		</rdfs:subClassOf>
		<rdfs:label>general ledger</rdfs:label>
		<skos:definition>accounting record summarizing changes in position as transactions are posted during an accounting period</skos:definition>
	</owl:Class>
	
	<owl:Class rdf:about="&fibo-fbc-pas-caa;InternationalBankAccountIdentifier">
		<rdfs:subClassOf rdf:resource="&fibo-fbc-pas-caa;BankAccountIdentifier"/>
		<rdfs:subClassOf>
			<owl:Restriction>
				<owl:onProperty rdf:resource="&fibo-fnd-rel-rel;comprises"/>
				<owl:onClass rdf:resource="&fibo-fbc-pas-caa;BasicBankAccountIdentifier"/>
				<owl:qualifiedCardinality rdf:datatype="&xsd;nonNegativeInteger">1</owl:qualifiedCardinality>
			</owl:Restriction>
		</rdfs:subClassOf>
		<rdfs:subClassOf>
			<owl:Restriction>
				<owl:onProperty rdf:resource="&fibo-fnd-rel-rel;comprises"/>
				<owl:onClass rdf:resource="&lcc-cr;Alpha2Code"/>
				<owl:qualifiedCardinality rdf:datatype="&xsd;nonNegativeInteger">1</owl:qualifiedCardinality>
			</owl:Restriction>
		</rdfs:subClassOf>
		<rdfs:subClassOf>
			<owl:Restriction>
				<owl:onProperty rdf:resource="&fibo-fnd-rel-rel;appliesTo"/>
				<owl:onClass rdf:resource="&lcc-cr;Country"/>
				<owl:qualifiedCardinality rdf:datatype="&xsd;nonNegativeInteger">1</owl:qualifiedCardinality>
			</owl:Restriction>
		</rdfs:subClassOf>
		<rdfs:label>international bank account identifier</rdfs:label>
		<skos:definition>identifier for a bank account that is an expanded version of the basic bank account number (BBAN), intended for use internationally</skos:definition>
		<fibo-fnd-utl-av:abbreviation>IBAN</fibo-fnd-utl-av:abbreviation>
		<fibo-fnd-utl-av:adaptedFrom>ISO 13616-1:2007 Financial services - International bank account number (IBAN)</fibo-fnd-utl-av:adaptedFrom>
		<fibo-fnd-utl-av:explanatoryNote>Note that international bank account numbers are formatted uniquely by country. A description of the country-specific formats is available from SWIFT (https://www.swift.com/), which is the ISO registrar for ISO 13616.</fibo-fnd-utl-av:explanatoryNote>
		<fibo-fnd-utl-av:synonym>international bank account number</fibo-fnd-utl-av:synonym>
	</owl:Class>
	
	<owl:Class rdf:about="&fibo-fbc-pas-caa;InvestmentAccount">
		<rdfs:subClassOf rdf:resource="&fibo-fbc-pas-caa;InvestmentOrDepositAccount"/>
		<rdfs:subClassOf>
			<owl:Restriction>
				<owl:onProperty rdf:resource="&fibo-fnd-rel-rel;isProvidedBy"/>
				<owl:someValuesFrom rdf:resource="&fibo-fbc-fct-fse;FinancialInstitution"/>
			</owl:Restriction>
		</rdfs:subClassOf>
		<rdfs:label>investment account</rdfs:label>
		<skos:definition>account that provides a record of deposits of funds and/or securities held at a financial institution</skos:definition>
		<fibo-fnd-utl-av:explanatoryNote>The typical objectives of an investment account are to achieve long term growth, income or capital preservation from the deposited asset portfolio.  Investment accounts are typically not insured.</fibo-fnd-utl-av:explanatoryNote>
	</owl:Class>
	
	<owl:Class rdf:about="&fibo-fbc-pas-caa;InvestmentOrDepositAccount">
		<rdfs:subClassOf rdf:resource="&fibo-fbc-pas-caa;FinancialServiceAccount"/>
		<rdfs:label>investment or deposit account</rdfs:label>
		<skos:definition>account associated with a product or service that requires the account holder to provide funds for management by the account provider</skos:definition>
		<fibo-fnd-utl-av:explanatoryNote>The account holder may or may not be entitled to consideration in exchange for providing such funds, for example, interest, depending on the type of account and the terms and conditions associated with it.  Also, there may be fees associated with management services provided by the account provider.</fibo-fnd-utl-av:explanatoryNote>
	</owl:Class>
	
	<owl:Class rdf:about="&fibo-fbc-pas-caa;LedgerAccount">
		<rdfs:subClassOf rdf:resource="&fibo-fbc-pas-caa;Account"/>
		<rdfs:label>ledger account</rdfs:label>
		<skos:definition>account recorded in a general ledger</skos:definition>
	</owl:Class>
	
	<owl:Class rdf:about="&fibo-fbc-pas-caa;LoanOrCreditAccount">
		<rdfs:subClassOf rdf:resource="&fibo-fbc-pas-caa;FinancialServiceAccount"/>
		<rdfs:label>loan or credit account</rdfs:label>
		<owl:disjointWith rdf:resource="&fibo-fbc-pas-caa;InvestmentOrDepositAccount"/>
		<skos:definition>account associated with a service in which the account holder receives funds from the account provider under certain terms and conditions for repayment</skos:definition>
	</owl:Class>
	
	<owl:Class rdf:about="&fibo-fbc-pas-caa;NonTransactionDepositAccount">
		<rdfs:subClassOf rdf:resource="&fibo-fbc-pas-caa;DepositAccount"/>
		<rdfs:label>non-transaction deposit account</rdfs:label>
		<owl:disjointWith rdf:resource="&fibo-fbc-pas-caa;TransactionDepositAccount"/>
		<skos:definition>any deposit account that is not explicitly considered a transaction account</skos:definition>
		<fibo-fnd-utl-av:adaptedFrom>https://www.fdic.gov/regulations/resources/call/crinst/2010-09/910gloss_093010.pdf</fibo-fnd-utl-av:adaptedFrom>
		<fibo-fnd-utl-av:explanatoryNote>Non-transaction accounts include: (a) savings deposits ((i) money market deposit accounts (MMDAs) and (ii) other savings deposits) and (b) time deposits ((i) time certificates of deposit and (ii) time deposits, open account).</fibo-fnd-utl-av:explanatoryNote>
	</owl:Class>
	
	<owl:Class rdf:about="&fibo-fbc-pas-caa;RelationshipManager">
		<rdfs:subClassOf rdf:resource="&fibo-be-oac-exec;ResponsibleParty"/>
		<rdfs:subClassOf>
			<owl:Restriction>
				<owl:onProperty rdf:resource="&fibo-fnd-rel-rel;manages"/>
				<owl:someValuesFrom rdf:resource="&fibo-fbc-pas-caa;Account"/>
			</owl:Restriction>
		</rdfs:subClassOf>
		<rdfs:label>relationship manager</rdfs:label>
		<skos:definition>responsible party who manages the client&apos;s account (or portfolio of accounts) and oversees their relationship with the service provider</skos:definition>
		<fibo-fnd-utl-av:synonym>account manager</fibo-fnd-utl-av:synonym>
	</owl:Class>
	
	<owl:Class rdf:about="&fibo-fbc-pas-caa;TimeCertificateOfDepositAccount">
		<rdfs:subClassOf rdf:resource="&fibo-fbc-pas-caa;TimeDepositAccount"/>
		<rdfs:subClassOf>
			<owl:Restriction>
				<owl:onProperty rdf:resource="&fibo-fbc-pas-caa;isRealizedBy"/>
				<owl:someValuesFrom rdf:resource="&fibo-fbc-pas-caa;CertificateOfDeposit"/>
			</owl:Restriction>
		</rdfs:subClassOf>
		<rdfs:label>time certificate of deposit account</rdfs:label>
		<skos:definition>time deposit account that allows deposits evidenced by a negotiable or nonnegotiable instrument, or a deposit in book entry form evidenced by a receipt or similar acknowledgement issued by the bank, that provides, on its face, that the amount of such deposit is payable to the bearer, to any specified person, or to the order of a specified person, as follows: (1) on a certain date not less than seven days after the date of deposit, (2) at the expiration of a specified period not less than seven days after the date of the deposit, or (3) upon written notice to the bank which is to be given not less than seven days before the date of withdrawal.</skos:definition>
		<fibo-fnd-utl-av:abbreviation>CDA</fibo-fnd-utl-av:abbreviation>
		<fibo-fnd-utl-av:adaptedFrom>https://www.fdic.gov/regulations/resources/call/crinst/2010-09/910gloss_093010.pdf</fibo-fnd-utl-av:adaptedFrom>
	</owl:Class>
	
	<owl:Class rdf:about="&fibo-fbc-pas-caa;TimeDepositAccount">
		<rdfs:subClassOf rdf:resource="&fibo-fbc-pas-caa;NonTransactionDepositAccount"/>
		<rdfs:subClassOf rdf:resource="&fibo-fnd-pas-pas;ContractualProduct"/>
		<rdfs:label>time deposit account</rdfs:label>
		<skos:definition>deposit account that the depositor does not have a right, and is not permitted, to make withdrawals from within six days after the date of deposit unless the deposit is subject to an early withdrawal penalty of at least seven days&apos; simple interest on amounts withdrawn within the first six days after deposit</skos:definition>
		<fibo-fnd-utl-av:adaptedFrom>https://www.fdic.gov/regulations/resources/call/crinst/2010-09/910gloss_093010.pdf</fibo-fnd-utl-av:adaptedFrom>
		<fibo-fnd-utl-av:explanatoryNote>A time deposit from which partial early withdrawals are permitted must impose additional early withdrawal penalties of at least seven days&apos; simple interest on amounts withdrawn within six days after each partial withdrawal. If such additional early withdrawal penalties are not imposed, the account ceases to be a time deposit. The account may become a savings deposit if it meets the requirements for a savings deposit; otherwise it becomes a demand deposit.</fibo-fnd-utl-av:explanatoryNote>
	</owl:Class>
	
	<owl:Class rdf:about="&fibo-fbc-pas-caa;TimeDepositOpenAccount">
		<rdfs:subClassOf rdf:resource="&fibo-fbc-pas-caa;TimeDepositAccount"/>
		<rdfs:label>time deposit open account</rdfs:label>
		<owl:disjointWith rdf:resource="&fibo-fbc-pas-caa;TimeCertificateOfDepositAccount"/>
		<skos:definition>time deposit account that allows deposits (other than time certificates of deposit) for which there is in force a written contract with the depositor that neither the whole nor any part of such deposit may be withdrawn prior to (1) the date of maturity which shall be not less than seven days after the date of the deposit, or (2) the expiration of a specified period of written notice of not less than seven days.</skos:definition>
		<fibo-fnd-utl-av:adaptedFrom>https://www.fdic.gov/regulations/resources/call/crinst/2010-09/910gloss_093010.pdf</fibo-fnd-utl-av:adaptedFrom>
	</owl:Class>
	
	<owl:Class rdf:about="&fibo-fbc-pas-caa;TransactionDepositAccount">
		<rdfs:subClassOf rdf:resource="&fibo-fbc-pas-caa;DepositAccount"/>
		<rdfs:label>transaction deposit account</rdfs:label>
		<skos:definition>deposit or account from which the depositor or account holder is permitted to make transfers or withdrawals by negotiable or transferable instruments, payment orders of withdrawal, telephone transfers, or other similar devices for the purpose of making payments or transfers to third persons or others or from which the depositor may make third party payments at an automated teller machine (ATM), a remote service unit (RSU), or another electronic device, including by debit card</skos:definition>
		<fibo-fnd-utl-av:adaptedFrom>https://www.fdic.gov/regulations/resources/call/crinst/2010-09/910gloss_093010.pdf</fibo-fnd-utl-av:adaptedFrom>
		<fibo-fnd-utl-av:explanatoryNote>Excluded from transaction accounts are savings deposits (both money market deposit accounts (MMDAs) and other savings deposits), even though such deposits permit some third-party transfers. However, an account that otherwise meets the definition of a savings deposit but that authorizes or permits the depositor to exceed the transfer limitations specified for that account shall be reported as a transaction account.</fibo-fnd-utl-av:explanatoryNote>
	</owl:Class>
	
	<owl:ObjectProperty rdf:about="&fibo-fbc-pas-caa;hasAccountCloseDate">
		<rdfs:subPropertyOf rdf:resource="&fibo-fnd-dt-fd;hasEndDate"/>
		<rdfs:label>has account close date</rdfs:label>
		<rdfs:domain rdf:resource="&fibo-fbc-pas-caa;Account"/>
		<rdfs:range rdf:resource="&fibo-fnd-dt-fd;ExplicitDate"/>
		<skos:definition>relates an account to the date that it was closed</skos:definition>
	</owl:ObjectProperty>
	
	<owl:ObjectProperty rdf:about="&fibo-fbc-pas-caa;hasAccountOpenDate">
		<rdfs:subPropertyOf rdf:resource="&fibo-fnd-dt-fd;hasStartDate"/>
		<rdfs:label>has account open date</rdfs:label>
		<rdfs:domain rdf:resource="&fibo-fbc-pas-caa;Account"/>
		<rdfs:range rdf:resource="&fibo-fnd-dt-fd;ExplicitDate"/>
		<skos:definition>relates an account to the date that it was created or opened</skos:definition>
	</owl:ObjectProperty>
	
	<owl:ObjectProperty rdf:about="&fibo-fbc-pas-caa;hasBalance">
		<rdfs:subPropertyOf rdf:resource="&fibo-fnd-acc-cur;hasMonetaryAmount"/>
		<rdfs:label>has balance</rdfs:label>
		<rdfs:domain rdf:resource="&fibo-fbc-pas-caa;Account"/>
		<rdfs:range rdf:resource="&fibo-fbc-pas-caa;Balance"/>
		<skos:definition>relates an account to the net amount of money available in that account</skos:definition>
	</owl:ObjectProperty>
	
	<owl:ObjectProperty rdf:about="&fibo-fbc-pas-caa;isRealizedBy">
		<rdfs:label>is realized by</rdfs:label>
		<owl:inverseOf rdf:resource="&fibo-fbc-pas-caa;realizes"/>
		<skos:definition>is made concrete by</skos:definition>
	</owl:ObjectProperty>
	
	<owl:ObjectProperty rdf:about="&fibo-fbc-pas-caa;realizes">
		<rdfs:subPropertyOf rdf:resource="&fibo-fnd-rel-rel;appliesTo"/>
		<rdfs:label>realizes</rdfs:label>
		<skos:definition>makes concrete</skos:definition>
	</owl:ObjectProperty>
	
	<owl:Class rdf:about="&fibo-fnd-pas-pas;ContractualProduct">
		<rdfs:subClassOf>
			<owl:Restriction>
				<owl:onProperty rdf:resource="&fibo-fbc-pas-caa;isRealizedBy"/>
				<owl:someValuesFrom rdf:resource="&fibo-fnd-agr-ctr;Contract"/>
			</owl:Restriction>
		</rdfs:subClassOf>
	</owl:Class>

</rdf:RDF>