<?xml version="1.0" encoding="UTF-8"?>
  
<!DOCTYPE rdf:RDF [
    <!ENTITY fibo-sec-dbt-dbt-cfl "http://spec.edmcouncil.org/fibo/red/sec/debt/debt-foundations/debt-cashflow-terms/">
    <!ENTITY fibo-fnd-acc-dbt "http://spec.edmcouncil.org/fibo/red/fnd/accounting/debt-terms/">
    <!ENTITY fibo-fnd-tim-tim "http://spec.edmcouncil.org/fibo/red/fnd/date-time/date-time/">
    <!ENTITY fibo-fnd-math-math "http://spec.edmcouncil.org/fibo/red/fnd/math/math/">
    <!ENTITY fibo-fnd-occ-evt "http://spec.edmcouncil.org/fibo/red/fnd/occurrent/events/">
    <!ENTITY fibo-fnd-agr-ctr "http://spec.edmcouncil.org/fibo/red/fnd/agreements/contracts/">
    <!ENTITY fibo-fnd-utl-bt "http://spec.edmcouncil.org/fibo/red/fnd/utilities/business-facing-types/">
    <!ENTITY fibo-fnd-agrx-ele "http://spec.edmcouncil.org/fibo/red/fnd/agreements-ext/contract-elements/">
    <!ENTITY fibo-sec-dbt-dbt-ins "http://spec.edmcouncil.org/fibo/red/sec/debt/debt-foundations/debt-instruments/">
    <!ENTITY fibo-sec-dbt-bond-cfl "http://spec.edmcouncil.org/fibo/red/sec/debt/bonds/bonds-cashflow-terms/">
    <!ENTITY fibo-ind-ind-ind "http://spec.edmcouncil.org/fibo/red/ind/indicators/indicators/">
    <!ENTITY fibo-der-ctr-exc "http://spec.edmcouncil.org/fibo/red/der/derivatives-contracts/exercise-conventions/">
    <!ENTITY fibo-der-ctr-opt "http://spec.edmcouncil.org/fibo/red/der/derivatives-contracts/options/">
    <!ENTITY fibo-uo-rl "http://spec.edmcouncil.org/fibo/red/uo/relatives/">
    <!ENTITY fibo-sec-sec-sec "http://spec.edmcouncil.org/fibo/red/sec/securities/securities/">
]>

<rdf:RDF xmlns:xsd="http://www.w3.org/2001/XMLSchema#"
         xmlns:sm="http://www.omg.org/techprocess/ab/SpecificationMetadata/"
         xmlns:xs="http://www.w3.org/2001/XMLSchema"
         xmlns:fibo-fnd-utl-av="http://www.omg.org/spec/EDMC-FIBO/FND/Utilities/AnnotationVocabulary/"
         xmlns:rdf="http://www.w3.org/1999/02/22-rdf-syntax-ns#"
         xmlns:rdfs="http://www.w3.org/2000/01/rdf-schema#"
         xmlns:owl="http://www.w3.org/2002/07/owl#"
         xmlns:skos="http://www.w3.org/2004/02/skos/core#"
         xmlns:dc="http://purl.org/dc/terms/"
         xml:base="http://spec.edmcouncil.org/fibo/red/sec/debt/debt-foundations/debt-cashflow-terms/">

   <owl:Ontology rdf:about="http://spec.edmcouncil.org/fibo/red/sec/debt/debt-foundations/debt-cashflow-terms/">
      <owl:imports rdf:resource="http://spec.edmcouncil.org/fibo/red/fnd/accounting/debt-terms/"/>
      <owl:imports rdf:resource="http://spec.edmcouncil.org/fibo/red/fnd/date-time/date-time/"/>
      <owl:imports rdf:resource="http://spec.edmcouncil.org/fibo/red/fnd/math/math/"/>
      <owl:imports rdf:resource="http://spec.edmcouncil.org/fibo/red/fnd/occurrent/events/"/>
      <owl:imports rdf:resource="http://spec.edmcouncil.org/fibo/red/fnd/agreements/contracts/"/>
      <owl:imports rdf:resource="http://spec.edmcouncil.org/fibo/red/fnd/utilities/business-facing-types/"/>
      <owl:imports rdf:resource="http://spec.edmcouncil.org/fibo/red/fnd/agreements-ext/contract-elements/"/>
      <owl:imports rdf:resource="http://spec.edmcouncil.org/fibo/red/sec/debt/debt-foundations/debt-instruments/"/>
      <owl:imports rdf:resource="http://spec.edmcouncil.org/fibo/red/sec/debt/bonds/bonds-cashflow-terms/"/>
      <owl:imports rdf:resource="http://spec.edmcouncil.org/fibo/red/ind/indicators/indicators/"/>
      <owl:imports rdf:resource="http://spec.edmcouncil.org/fibo/red/der/derivatives-contracts/exercise-conventions/"/>
      <owl:imports rdf:resource="http://spec.edmcouncil.org/fibo/red/der/derivatives-contracts/options/"/>
      <owl:imports rdf:resource="http://spec.edmcouncil.org/fibo/red/uo/relatives/"/>
      <owl:imports rdf:resource="http://spec.edmcouncil.org/fibo/red/sec/securities/securities/"/>
   </owl:Ontology>


  <!--
    ///////////////////////////////////////////////////////////////////////////////////////
    //
    // Datatypes
    //
    ///////////////////////////////////////////////////////////////////////////////////////
    -->


<rdfs:Datatype rdf:about="&fibo-sec-dbt-dbt-cfl;CallType">
      <skos:definition>Way in which a call will be executed, which is by Lottery or Pro-Rata.</skos:definition>
      <owl:equivalentClass>
         <rdfs:Datatype>
            <owl:oneOf>
               <rdf:Description>
                  <rdf:first rdf:datatype="http://www.w3.org/2001/XMLSchema#string">Pro Rata</rdf:first>
                  <rdf:rest>
                     <rdf:Description>
                        <rdf:first rdf:datatype="http://www.w3.org/2001/XMLSchema#string">Lottery</rdf:first>
                        <rdf:rest rdf:resource="http://www.w3.org/1999/02/22-rdf-syntax-ns#nil"/>
                     </rdf:Description>
                  </rdf:rest>
               </rdf:Description>
            </owl:oneOf>
         </rdfs:Datatype>
      </owl:equivalentClass>
   </rdfs:Datatype>


  <!--
    ///////////////////////////////////////////////////////////////////////////////////////
    //
    // Object Properties
    //
    ///////////////////////////////////////////////////////////////////////////////////////
    -->


<owl:ObjectProperty rdf:about="&fibo-sec-dbt-dbt-cfl;operand">
      <rdfs:label>operand</rdfs:label>
      <rdfs:subPropertyOf rdf:resource="&fibo-fnd-math-math;operand"/>
      <rdfs:domain rdf:resource="&fibo-sec-dbt-dbt-cfl;Base"/>
      <rdfs:range rdf:resource="&fibo-ind-ind-ind;MarketReferentialParameter"/>
   </owl:ObjectProperty>

   <owl:ObjectProperty rdf:about="&fibo-sec-dbt-dbt-cfl;schedulesPossibleEvent">
      <rdfs:label>schedules possible event</rdfs:label>
      <rdfs:subPropertyOf rdf:resource="&fibo-fnd-tim-tim;scheduledEvent"/>
      <rdfs:domain rdf:resource="&fibo-sec-dbt-dbt-cfl;CallScheduleListing"/>
      <rdfs:range rdf:resource="&fibo-sec-dbt-bond-cfl;CallOfIssue"/>
   </owl:ObjectProperty>

   <owl:ObjectProperty rdf:about="&fibo-sec-dbt-dbt-cfl;expressedAs">
      <rdfs:label>expressed as</rdfs:label>
      <rdfs:subPropertyOf rdf:resource="&fibo-fnd-tim-tim;expressedAs"/>
      <rdfs:domain rdf:resource="&fibo-sec-dbt-dbt-cfl;CallSchedule"/>
      <rdfs:range rdf:resource="&fibo-sec-dbt-dbt-cfl;CallScheduleListing"/>
   </owl:ObjectProperty>

   <owl:ObjectProperty rdf:about="&fibo-sec-dbt-dbt-cfl;callTermsExerciseOptionsDetails">
      <rdfs:label>call terms exercise options details</rdfs:label>
      <rdfs:domain rdf:resource="&fibo-sec-dbt-dbt-cfl;DebtCallTermsSet"/>
      <rdfs:range rdf:resource="&fibo-der-ctr-exc;ExerciseDatesConvention"/>
   </owl:ObjectProperty>

   <owl:ObjectProperty rdf:about="&fibo-sec-dbt-dbt-cfl;includesSchedule">
      <rdfs:label>includes schedule</rdfs:label>
      <rdfs:subPropertyOf rdf:resource="&fibo-fnd-agrx-ele;hasTerm"/>
      <rdfs:domain rdf:resource="&fibo-sec-dbt-dbt-cfl;DebtCallTermsSet"/>
      <rdfs:range rdf:resource="&fibo-sec-dbt-dbt-cfl;CallSchedule"/>
   </owl:ObjectProperty>

   <owl:ObjectProperty rdf:about="&fibo-sec-dbt-dbt-cfl;includesWindow">
      <rdfs:label>includes window</rdfs:label>
      <rdfs:subPropertyOf rdf:resource="&fibo-fnd-agrx-ele;hasTerm"/>
      <rdfs:domain rdf:resource="&fibo-sec-dbt-dbt-cfl;DebtCallTermsSet"/>
      <rdfs:range rdf:resource="&fibo-sec-dbt-dbt-cfl;CallWindow"/>
   </owl:ObjectProperty>

   <owl:ObjectProperty rdf:about="&fibo-sec-dbt-dbt-cfl;calendar">
      <rdfs:label>calendar</rdfs:label>
      <rdfs:subPropertyOf rdf:resource="&fibo-fnd-tim-tim;denominatedIn"/>
      <rdfs:domain rdf:resource="&fibo-sec-dbt-dbt-cfl;CallWindow"/>
      <rdfs:range rdf:resource="&fibo-sec-dbt-dbt-cfl;.UnionClass.4"/>
   </owl:ObjectProperty>

   <owl:ObjectProperty rdf:about="&fibo-sec-dbt-dbt-cfl;compoundingFrequency">
      <rdfs:label>compounding frequency</rdfs:label>
      <skos:definition>The frequency at which the interest is compounded. This is established at the initial stages of securing the instrument. Generally, interest tends to be calculated on an annual basis although other terms may be established at the time of the loan.</skos:definition>
      <rdfs:domain rdf:resource="&fibo-sec-dbt-dbt-cfl;DebtSecurityInterestPaymentTermsSet"/>
      <rdfs:range rdf:resource="&fibo-fnd-tim-tim;Frequency"/>
   </owl:ObjectProperty>

   <owl:ObjectProperty rdf:about="&fibo-sec-dbt-dbt-cfl;interestPaymentFrequency">
      <rdfs:label>interest payment frequency</rdfs:label>
      <skos:definition>Frequency of payment of Interest on the debt.</skos:definition>
      <rdfs:domain rdf:resource="&fibo-sec-dbt-dbt-cfl;DebtSecurityInterestPaymentTermsSet"/>
      <rdfs:range rdf:resource="&fibo-fnd-tim-tim;Frequency"/>
   </owl:ObjectProperty>

   <owl:ObjectProperty rdf:about="&fibo-sec-dbt-dbt-cfl;extendableDate">
      <rdfs:label>extendable date</rdfs:label>
      <skos:definition>Date to which the Maturity Date may be extended. This date is determined at the set-up of the bond. Note this date is adjustable according to various applicable parameters or terms. May have a rolling extendable maturity date. The bond holder may choose to extend. Usually a 13 month rolling extendable maturity.</skos:definition>
      <rdfs:domain rdf:resource="&fibo-sec-dbt-dbt-cfl;ExtendableMaturityRedemptionTermsSet"/>
      <rdfs:range rdf:resource="&fibo-fnd-tim-tim;DeterminedDate"/>
   </owl:ObjectProperty>

   <owl:ObjectProperty rdf:about="&fibo-sec-dbt-dbt-cfl;extendablePeriod">
      <rdfs:label>extendable period</rdfs:label>
      <skos:definition>Period during which the Maturity Date may be extended.</skos:definition>
      <rdfs:domain rdf:resource="&fibo-sec-dbt-dbt-cfl;ExtendableMaturityRedemptionTermsSet"/>
      <rdfs:range rdf:resource="&fibo-fnd-tim-tim;DatePeriod"/>
   </owl:ObjectProperty>

   <owl:ObjectProperty rdf:about="&fibo-sec-dbt-dbt-cfl;hasBaseParameter">
      <rdfs:label>has base parameter</rdfs:label>
      <rdfs:subPropertyOf rdf:resource="&fibo-fnd-math-math;hasArgument"/>
      <rdfs:domain rdf:resource="&fibo-sec-dbt-dbt-cfl;InterestCalculationExpression"/>
      <rdfs:range rdf:resource="&fibo-sec-dbt-dbt-cfl;Base"/>
   </owl:ObjectProperty>

   <owl:ObjectProperty rdf:about="&fibo-sec-dbt-dbt-cfl;hasMarginParameter">
      <rdfs:label>has margin parameter</rdfs:label>
      <rdfs:subPropertyOf rdf:resource="&fibo-fnd-math-math;hasArgument"/>
      <rdfs:domain rdf:resource="&fibo-sec-dbt-dbt-cfl;InterestCalculationExpression"/>
      <rdfs:range rdf:resource="&fibo-sec-dbt-dbt-cfl;Margin"/>
   </owl:ObjectProperty>

   <owl:ObjectProperty rdf:about="&fibo-sec-dbt-dbt-cfl;expression.1">
      <rdfs:label>expression</rdfs:label>
      <rdfs:subPropertyOf rdf:resource="&fibo-fnd-math-math;expression.1"/>
      <rdfs:domain rdf:resource="&fibo-sec-dbt-dbt-cfl;InterestCalculationFormula"/>
      <rdfs:range rdf:resource="&fibo-sec-dbt-dbt-cfl;InterestCalculationExpression"/>
   </owl:ObjectProperty>

   <owl:ObjectProperty rdf:about="&fibo-sec-dbt-dbt-cfl;subject">
      <rdfs:label>subject</rdfs:label>
      <rdfs:subPropertyOf rdf:resource="&fibo-fnd-math-math;subject"/>
      <rdfs:domain rdf:resource="&fibo-sec-dbt-dbt-cfl;InterestCalculationFormula"/>
      <rdfs:range rdf:resource="&fibo-sec-dbt-dbt-cfl;InterestCalculationSubject"/>
   </owl:ObjectProperty>

   <owl:ObjectProperty rdf:about="&fibo-sec-dbt-dbt-cfl;subjectIs">
      <rdfs:label>subject is</rdfs:label>
      <rdfs:subPropertyOf rdf:resource="&fibo-uo-rl;identity"/>
      <rdfs:domain rdf:resource="&fibo-sec-dbt-dbt-cfl;InterestCalculationSubject"/>
      <rdfs:range rdf:resource="&fibo-sec-dbt-dbt-cfl;SecuritizedDebtInterest"/>
   </owl:ObjectProperty>

   <owl:ObjectProperty rdf:about="&fibo-sec-dbt-dbt-cfl;hasTerm">
      <rdfs:label>has term</rdfs:label>
      <rdfs:subPropertyOf rdf:resource="&fibo-fnd-agrx-ele;hasTerm"/>
      <rdfs:domain rdf:resource="&fibo-sec-dbt-dbt-cfl;DebtSecurityInterestPaymentTermsSet"/>
      <rdfs:range rdf:resource="&fibo-sec-dbt-dbt-cfl;InterestCalculationFormula"/>
   </owl:ObjectProperty>

   <owl:ObjectProperty rdf:about="&fibo-sec-dbt-dbt-cfl;hasCallTerms">
      <rdfs:label>has call terms</rdfs:label>
      <rdfs:subPropertyOf rdf:resource="&fibo-sec-dbt-dbt-ins;hasCallTerms"/>
      <rdfs:subPropertyOf rdf:resource="&fibo-fnd-agr-ctr;contractHasTerms"/>
      <rdfs:domain rdf:resource="&fibo-sec-dbt-dbt-ins;NonTradableDebtInstrument"/>
      <rdfs:range rdf:resource="&fibo-sec-dbt-dbt-cfl;DebtCallTermsSet"/>
   </owl:ObjectProperty>

   <owl:ObjectProperty rdf:about="&fibo-sec-dbt-dbt-cfl;putFrequency">
      <rdfs:label>put frequency</rdfs:label>
      <skos:definition>Frequency of Tender or Put period.</skos:definition>
      <rdfs:domain rdf:resource="&fibo-sec-dbt-dbt-cfl;PutTermsSet"/>
      <rdfs:range rdf:resource="&fibo-fnd-tim-tim;Frequency"/>
   </owl:ObjectProperty>

   <owl:ObjectProperty rdf:about="&fibo-sec-dbt-dbt-cfl;includes">
      <rdfs:label>includes</rdfs:label>
      <rdfs:subPropertyOf rdf:resource="&fibo-fnd-agrx-ele;hasTerm"/>
      <rdfs:domain rdf:resource="&fibo-sec-dbt-dbt-cfl;PutTermsSet"/>
      <rdfs:range rdf:resource="&fibo-sec-dbt-dbt-cfl;PutSchedule"/>
   </owl:ObjectProperty>

   <owl:ObjectProperty rdf:about="&fibo-sec-dbt-dbt-cfl;includesWindow.1">
      <rdfs:label>includes window</rdfs:label>
      <rdfs:subPropertyOf rdf:resource="&fibo-fnd-agrx-ele;hasTerm"/>
      <rdfs:domain rdf:resource="&fibo-sec-dbt-dbt-cfl;PutTermsSet"/>
      <rdfs:range rdf:resource="&fibo-sec-dbt-dbt-cfl;PutWindow"/>
   </owl:ObjectProperty>

   <owl:ObjectProperty rdf:about="&fibo-sec-dbt-dbt-cfl;calendar.1">
      <rdfs:label>calendar</rdfs:label>
      <rdfs:subPropertyOf rdf:resource="&fibo-fnd-tim-tim;denominatedIn"/>
      <rdfs:domain rdf:resource="&fibo-sec-dbt-dbt-cfl;PutWindow"/>
      <rdfs:range rdf:resource="&fibo-sec-dbt-dbt-cfl;.UnionClass.4"/>
   </owl:ObjectProperty>

   <owl:ObjectProperty rdf:about="&fibo-sec-dbt-dbt-cfl;hasCallTerms.1">
      <rdfs:label>has call terms</rdfs:label>
      <rdfs:subPropertyOf rdf:resource="&fibo-fnd-agr-ctr;contractHasTerms"/>
      <rdfs:domain rdf:resource="&fibo-sec-dbt-dbt-ins;TradableDebtInstrument"/>
      <rdfs:range rdf:resource="&fibo-sec-dbt-dbt-cfl;DebtCallTermsSet"/>
   </owl:ObjectProperty>

   <owl:ObjectProperty rdf:about="&fibo-sec-dbt-dbt-cfl;includesForExtendableMaturity">
      <rdfs:label>includes for extendable maturity</rdfs:label>
      <skos:definition>In the case of terms where extendable maturity is yes, terms are included regarding the extension of the maturity on the security.</skos:definition>
      <rdfs:subPropertyOf rdf:resource="&fibo-fnd-agr-ctr;contractTermsSetHasPart"/>
      <rdfs:domain rdf:resource="&fibo-sec-dbt-dbt-cfl;TradableDebtSecurityRedemptionTermsSet"/>
      <rdfs:range rdf:resource="&fibo-sec-dbt-dbt-cfl;ExtendableMaturityRedemptionTermsSet"/>
   </owl:ObjectProperty>

   <owl:ObjectProperty rdf:about="&fibo-sec-dbt-dbt-cfl;hasInterestTerms">
      <rdfs:label>has interest terms</rdfs:label>
      <rdfs:subPropertyOf rdf:resource="&fibo-fnd-agr-ctr;contractHasTerms"/>
      <rdfs:domain rdf:resource="&fibo-sec-dbt-dbt-ins;TradableDebtInstrument"/>
      <rdfs:range rdf:resource="&fibo-sec-dbt-dbt-cfl;DebtSecurityInterestPaymentTermsSet"/>
   </owl:ObjectProperty>

   <owl:ObjectProperty rdf:about="&fibo-sec-dbt-dbt-cfl;hasPrincipalTerms">
      <rdfs:label>has principal terms</rdfs:label>
      <rdfs:subPropertyOf rdf:resource="&fibo-fnd-agr-ctr;contractHasTerms"/>
      <rdfs:domain rdf:resource="&fibo-sec-dbt-dbt-ins;TradableDebtInstrument"/>
      <rdfs:range rdf:resource="&fibo-sec-dbt-dbt-cfl;TradableDebtSecurityRedemptionTermsSet"/>
   </owl:ObjectProperty>


  <!--
    ///////////////////////////////////////////////////////////////////////////////////////
    //
    // Data Properties
    //
    ///////////////////////////////////////////////////////////////////////////////////////
    -->


<owl:DatatypeProperty rdf:about="&fibo-sec-dbt-dbt-cfl;roundingDecimalPlaces">
      <rdfs:label>rounding decimal places</rdfs:label>
      <skos:definition>Number of decimal places to round to.</skos:definition>
      <rdfs:range rdf:resource="&fibo-fnd-utl-bt;wholeNumber"/>
   </owl:DatatypeProperty>

   <owl:DatatypeProperty rdf:about="&fibo-sec-dbt-dbt-cfl;truncatingDecimalPlaces">
      <rdfs:label>truncating decimal places</rdfs:label>
      <skos:definition>Number of decimal places. Note this is either/or with the Rounding number of decimal places.</skos:definition>
      <rdfs:range rdf:resource="&fibo-fnd-utl-bt;wholeNumber"/>
   </owl:DatatypeProperty>

   <owl:DatatypeProperty rdf:about="&fibo-sec-dbt-dbt-cfl;discrete">
      <rdfs:label>discrete</rdfs:label>
      <skos:definition>Whether calls are discrete or continuous. No = continuous.</skos:definition>
      <rdfs:range rdf:resource="&fibo-fnd-utl-bt;yesOrNo"/>
   </owl:DatatypeProperty>

   <owl:DatatypeProperty rdf:about="&fibo-sec-dbt-dbt-cfl;notification">
      <rdfs:label>notification</rdfs:label>
      <skos:definition>Whether Call Schedule includes notification.</skos:definition>
      <rdfs:range rdf:resource="&fibo-fnd-utl-bt;yesOrNo"/>
   </owl:DatatypeProperty>

   <owl:DatatypeProperty rdf:about="&fibo-sec-dbt-dbt-cfl;daysToCallNotification">
      <rdfs:label>days to call notification</rdfs:label>
      <skos:definition>Number of days prior to a call date that the issuer/agent must give notice to holders.</skos:definition>
      <rdfs:range rdf:resource="&fibo-fnd-utl-bt;wholeNumber"/>
   </owl:DatatypeProperty>

   <owl:DatatypeProperty rdf:about="&fibo-sec-dbt-dbt-cfl;callExerciseDateTerms">
      <rdfs:label>call exercise date terms</rdfs:label>
      <skos:definition>The specific date windows when a debt security can be called back by the issuer.</skos:definition>
      <rdfs:range rdf:resource="&fibo-der-ctr-opt;ExerciseOptions"/>
   </owl:DatatypeProperty>

   <owl:DatatypeProperty rdf:about="&fibo-sec-dbt-dbt-cfl;callType">
      <rdfs:label>call type</rdfs:label>
      <skos:definition>Whether the call will be executed by Lottery or Pro-Rata.</skos:definition>
      <rdfs:range rdf:resource="&fibo-sec-dbt-dbt-cfl;CallType"/>
   </owl:DatatypeProperty>

   <owl:DatatypeProperty rdf:about="&fibo-sec-dbt-dbt-cfl;extraordinaryCallProvision">
      <rdfs:label>extraordinary call provision</rdfs:label>
      <skos:definition>Indicates the existence of an Extraordinary Call provision in the bond call terms.</skos:definition>
      <rdfs:range rdf:resource="&fibo-fnd-utl-bt;yesOrNo"/>
   </owl:DatatypeProperty>

   <owl:DatatypeProperty rdf:about="&fibo-sec-dbt-dbt-cfl;firstParCallDate">
      <rdfs:label>first par call date</rdfs:label>
      <skos:definition>The first date on which bonds may be called at Par for redemption.</skos:definition>
      <rdfs:range rdf:resource="http://www.w3.org/2001/XMLSchema#date"/>
   </owl:DatatypeProperty>

   <owl:DatatypeProperty rdf:about="&fibo-sec-dbt-dbt-cfl;firstParCallPrice">
      <rdfs:label>first par call price</rdfs:label>
      <skos:definition>The price of the bonds on the first Par part call.</skos:definition>
      <rdfs:range rdf:resource="&fibo-fnd-utl-bt;percentage"/>
   </owl:DatatypeProperty>

   <owl:DatatypeProperty rdf:about="&fibo-sec-dbt-dbt-cfl;firstPremiumCallDate">
      <rdfs:label>first premium call date</rdfs:label>
      <skos:definition>The first date on which bonds may be called for redemption at a price above par.</skos:definition>
      <rdfs:range rdf:resource="http://www.w3.org/2001/XMLSchema#date"/>
   </owl:DatatypeProperty>

   <owl:DatatypeProperty rdf:about="&fibo-sec-dbt-dbt-cfl;firstPremiumCallPrice">
      <rdfs:label>first premium call price</rdfs:label>
      <skos:definition>The price of the bonds on the first part call at a price above par.</skos:definition>
      <rdfs:range rdf:resource="&fibo-fnd-utl-bt;percentage"/>
   </owl:DatatypeProperty>

   <owl:DatatypeProperty rdf:about="&fibo-sec-dbt-dbt-cfl;makeWholeCallProvision">
      <rdfs:label>make whole call provision</rdfs:label>
      <skos:definition>A provision on the bond allowing the borrower to pay off remaining debt early.</skos:definition>
      <rdfs:range rdf:resource="&fibo-fnd-utl-bt;yesOrNo"/>
   </owl:DatatypeProperty>

   <owl:DatatypeProperty rdf:about="&fibo-sec-dbt-dbt-cfl;mandatorySinkingFund">
      <rdfs:label>mandatory sinking fund</rdfs:label>
      <skos:definition>Whether there is a Mandatory Sinking fund feature.</skos:definition>
      <rdfs:range rdf:resource="&fibo-fnd-utl-bt;yesOrNo"/>
   </owl:DatatypeProperty>

   <owl:DatatypeProperty rdf:about="&fibo-sec-dbt-dbt-cfl;accrualBasis">
      <rdfs:label>accrual basis</rdfs:label>
      <skos:definition>The number of days in a month and days in a year that are counted when performing interest accrual calculations.</skos:definition>
      <rdfs:range rdf:resource="&fibo-sec-dbt-dbt-ins;DayCountBasis"/>
   </owl:DatatypeProperty>

   <owl:DatatypeProperty rdf:about="&fibo-sec-dbt-dbt-cfl;autoReinvestment">
      <rdfs:label>auto reinvestment</rdfs:label>
      <skos:definition>Whether the security provides for mandatorily & automatically re-investing the interest from that security towards buying more of the same security.</skos:definition>
      <rdfs:range rdf:resource="&fibo-fnd-utl-bt;yesOrNo"/>
   </owl:DatatypeProperty>

   <owl:DatatypeProperty rdf:about="&fibo-sec-dbt-dbt-cfl;firstInterestAccrualDate">
      <rdfs:label>first interest accrual date</rdfs:label>
      <skos:definition>Date from which the security begins to accrue interest.</skos:definition>
      <rdfs:range rdf:resource="http://www.w3.org/2001/XMLSchema#date"/>
   </owl:DatatypeProperty>

   <owl:DatatypeProperty rdf:about="&fibo-sec-dbt-dbt-cfl;firstInterestPaymentDate">
      <rdfs:label>first interest payment date</rdfs:label>
      <skos:definition>The day on which the first interest payment is due to the holders of the security.</skos:definition>
      <rdfs:range rdf:resource="http://www.w3.org/2001/XMLSchema#date"/>
   </owl:DatatypeProperty>

   <owl:DatatypeProperty rdf:about="&fibo-sec-dbt-dbt-cfl;interestPaymentDayAndMonth">
      <rdfs:label>interest payment day and month</rdfs:label>
      <skos:definition>The regular dates of interest payment in any given year during the life of the debt instrument.</skos:definition>
      <rdfs:range rdf:resource="&fibo-fnd-utl-bt;dayAndMonth"/>
   </owl:DatatypeProperty>

   <owl:DatatypeProperty rdf:about="&fibo-sec-dbt-dbt-cfl;lastInterestPaymentDate">
      <rdfs:label>last interest payment date</rdfs:label>
      <skos:definition>The day on which the final interest payment is due to the holders of the security prior to maturity. This is only needed if the last coupon is of an odd length.</skos:definition>
      <rdfs:range rdf:resource="http://www.w3.org/2001/XMLSchema#date"/>
   </owl:DatatypeProperty>

   <owl:DatatypeProperty rdf:about="&fibo-sec-dbt-dbt-cfl;payInKind">
      <rdfs:label>pay in kind</rdfs:label>
      <skos:definition>The issuer will pay additional security as part of interest disbursement. Review: This needs to be replaced wit a sub class of Interst Payment in which the additional security is specified.</skos:definition>
      <rdfs:range rdf:resource="&fibo-fnd-utl-bt;yesOrNo"/>
   </owl:DatatypeProperty>

   <owl:DatatypeProperty rdf:about="&fibo-sec-dbt-dbt-cfl;proRated">
      <rdfs:label>pro rated</rdfs:label>
      <skos:definition>Whether the coupon is pro rated to the actual number of days in the payment period versus the number of payment periods.</skos:definition>
      <rdfs:range rdf:resource="&fibo-fnd-utl-bt;yesOrNo"/>
   </owl:DatatypeProperty>

   <owl:DatatypeProperty rdf:about="&fibo-sec-dbt-dbt-cfl;expression">
      <rdfs:label>expression</rdfs:label>
      <skos:definition>Textual expression of the entire right hand side of the Formula. Note that this is additional to the modelling of the separate Arguments that make up the formula.</skos:definition>
      <rdfs:range rdf:resource="&fibo-fnd-utl-bt;text"/>
   </owl:DatatypeProperty>

   <owl:DatatypeProperty rdf:about="&fibo-sec-dbt-dbt-cfl;amount">
      <rdfs:label>amount</rdfs:label>
      <skos:definition>A fixed, constant amount which forms the Margin parameter, expressed as a percentage.</skos:definition>
      <rdfs:range rdf:resource="&fibo-fnd-utl-bt;percentage"/>
   </owl:DatatypeProperty>

   <owl:DatatypeProperty rdf:about="&fibo-sec-dbt-dbt-cfl;interestRate">
      <rdfs:label>interest rate</rdfs:label>
      <skos:definition>The annual percentage rate of interest that must be paid on the debt.</skos:definition>
      <rdfs:range rdf:resource="&fibo-fnd-utl-bt;percentage"/>
   </owl:DatatypeProperty>

   <owl:DatatypeProperty rdf:about="&fibo-sec-dbt-dbt-cfl;daysToPut">
      <rdfs:label>days to put</rdfs:label>
      <skos:definition>Number of days prior to a mandatory or optional redemption date that the issuer/agent must give notice to holders.</skos:definition>
      <rdfs:range rdf:resource="&fibo-fnd-utl-bt;wholeNumber"/>
   </owl:DatatypeProperty>

   <owl:DatatypeProperty rdf:about="&fibo-sec-dbt-dbt-cfl;estateOrDeathPut">
      <rdfs:label>estate or death put</rdfs:label>
      <skos:definition>Specifies that a security is subject to be Redeemed upon the passing of the holder.</skos:definition>
      <rdfs:range rdf:resource="&fibo-fnd-utl-bt;yesOrNo"/>
   </owl:DatatypeProperty>

   <owl:DatatypeProperty rdf:about="&fibo-sec-dbt-dbt-cfl;putDate">
      <rdfs:label>put date</rdfs:label>
      <skos:definition>Date on which securities are subject to Optional or Mandatory Redemption by the bond holder.</skos:definition>
      <rdfs:range rdf:resource="http://www.w3.org/2001/XMLSchema#date"/>
   </owl:DatatypeProperty>

   <owl:DatatypeProperty rdf:about="&fibo-sec-dbt-dbt-cfl;putType">
      <rdfs:label>put type</rdfs:label>
      <skos:definition>Whether the redemption prior to maturity date feature is Mandatory or Optional to the bond holder.</skos:definition>
      <rdfs:range rdf:resource="&fibo-sec-sec-sec;Optionality"/>
   </owl:DatatypeProperty>

   <owl:DatatypeProperty rdf:about="&fibo-sec-dbt-dbt-cfl;rightToRetain">
      <rdfs:label>right to retain</rdfs:label>
      <skos:definition>Whether the holder has an option to retain the security in the event of an issuer exercising the put option.</skos:definition>
      <rdfs:range rdf:resource="&fibo-fnd-utl-bt;yesOrNo"/>
   </owl:DatatypeProperty>

   <owl:DatatypeProperty rdf:about="&fibo-sec-dbt-dbt-cfl;daysToPutNotification">
      <rdfs:label>days to put notification</rdfs:label>
      <skos:definition>Number of days prior to a mandatory or optional redemption date that the issuer/agent must give notice to holders. This term replaces the Multipler term in the Duratiojn Description.</skos:definition>
      <rdfs:range rdf:resource="&fibo-fnd-utl-bt;wholeNumber"/>
   </owl:DatatypeProperty>

   <owl:DatatypeProperty rdf:about="&fibo-sec-dbt-dbt-cfl;extendableByHolder">
      <rdfs:label>extendable by holder</rdfs:label>
      <skos:definition>Indicates whether the expiration date or maturity date can be extended by the holder, i.e. repayment may be extended or maturity changed.</skos:definition>
      <rdfs:range rdf:resource="&fibo-fnd-utl-bt;yesOrNo"/>
   </owl:DatatypeProperty>

   <owl:DatatypeProperty rdf:about="&fibo-sec-dbt-dbt-cfl;extendableByIssuer">
      <rdfs:label>extendable by issuer</rdfs:label>
      <skos:definition>Whether the issuer has the option to extend the debt rather than refinancing. If not, the issuer may only refinance the debt by calling the issue and creating a new issue.</skos:definition>
      <rdfs:range rdf:resource="&fibo-fnd-utl-bt;yesOrNo"/>
   </owl:DatatypeProperty>

   <owl:DatatypeProperty rdf:about="&fibo-sec-dbt-dbt-cfl;legalFinalMaturityDate">
      <rdfs:label>legal final maturity date</rdfs:label>
      <skos:definition>Date when the debt instrument is contractually obliged to mature. It is also the termination or due date on which an installment loan must be paid in full.</skos:definition>
      <rdfs:range rdf:resource="http://www.w3.org/2001/XMLSchema#date"/>
   </owl:DatatypeProperty>

   <owl:DatatypeProperty rdf:about="&fibo-sec-dbt-dbt-cfl;paymentInKind">
      <rdfs:label>payment in kind</rdfs:label>
      <skos:definition>Whether the Principal may be repaid in kind rather than in cash.</skos:definition>
      <rdfs:range rdf:resource="&fibo-fnd-utl-bt;yesOrNo"/>
   </owl:DatatypeProperty>

   <owl:DatatypeProperty rdf:about="&fibo-sec-dbt-dbt-cfl;perpetualMaturity">
      <rdfs:label>perpetual maturity</rdfs:label>
      <skos:definition>Whether the debt security has perpetual maturity, i.e. there is no Maturity Date and the security remains in issue indefinitely or until recalled.</skos:definition>
      <rdfs:range rdf:resource="&fibo-fnd-utl-bt;yesOrNo"/>
   </owl:DatatypeProperty>

   <owl:DatatypeProperty rdf:about="&fibo-sec-dbt-dbt-cfl;scheduledMaturityDate">
      <rdfs:label>scheduled maturity date</rdfs:label>
      <skos:definition>Originally specified date on which an interest bearing security becomes due and assets are to be repaid, as stated in the security's offering documents. This is the date on which the principal amount of a debt instrument becomes due and is repaid to the investor and interest payments stop.</skos:definition>
      <rdfs:range rdf:resource="http://www.w3.org/2001/XMLSchema#date"/>
   </owl:DatatypeProperty>


  <!--
    ///////////////////////////////////////////////////////////////////////////////////////
    //
    // Annotation Properties
    //
    ///////////////////////////////////////////////////////////////////////////////////////
    -->



  <!--
    ///////////////////////////////////////////////////////////////////////////////////////
    //
    // Classes
    //
    ///////////////////////////////////////////////////////////////////////////////////////
    -->


<owl:Class rdf:about="&fibo-sec-dbt-dbt-cfl;.UnionClass.4">
      <skos:definition>Calendar is defined in terms of either a Calendar Day or a Business Day.</skos:definition>
      <owl:equivalentClass>
         <owl:Class>
            <owl:unionOf rdf:parseType="Collection">
               <owl:Class rdf:about="&fibo-fnd-tim-tim;Day"/>
               <owl:Class rdf:about="&fibo-fnd-tim-tim;BusinessDay"/>
            </owl:unionOf>
         </owl:Class>
      </owl:equivalentClass>
   </owl:Class>

   <owl:Class rdf:about="&fibo-sec-dbt-dbt-cfl;Base">
      <rdfs:label>base</rdfs:label>
      <skos:definition>The variable to which an additional Margin amount is added to get the Interest amount.</skos:definition>
      <rdfs:subClassOf rdf:resource="&fibo-fnd-math-math;FormulaArgument"/>
   </owl:Class>

   <owl:Class rdf:about="&fibo-sec-dbt-dbt-cfl;CallSchedule">
      <rdfs:label>call schedule</rdfs:label>
      <rdfs:subClassOf rdf:resource="&fibo-fnd-tim-tim;Schedule"/>
   </owl:Class>

   <owl:Class rdf:about="&fibo-sec-dbt-dbt-cfl;CallScheduleListing">
      <rdfs:label>call schedule listing</rdfs:label>
      <skos:definition>Schedule fo dates on which a Traded Security can be Called (recalled) by the Issuer.</skos:definition>
      <rdfs:subClassOf rdf:resource="&fibo-fnd-tim-tim;ExplicitScheduleListing"/>
   </owl:Class>

   <owl:Class rdf:about="&fibo-sec-dbt-dbt-cfl;CallWindow">
      <rdfs:label>call window</rdfs:label>
      <skos:definition>Window of days prior to a call date that the issuer/agent must give notice to holders.</skos:definition>
      <rdfs:subClassOf rdf:resource="&fibo-fnd-tim-tim;DurationDescription"/>
   </owl:Class>

   <owl:Class rdf:about="&fibo-sec-dbt-dbt-cfl;DebtCallTermsSet">
      <rdfs:label>debt call terms set</rdfs:label>
      <rdfs:subClassOf rdf:resource="&fibo-sec-dbt-dbt-cfl;TradableDebtSecurityRedemptionTermsSet"/>
   </owl:Class>

   <owl:Class rdf:about="&fibo-sec-dbt-dbt-cfl;DebtSecurityInterestPaymentTermsSet">
      <rdfs:label>debt security interest payment terms set</rdfs:label>
      <skos:definition>Terms defining the interest or Coupon to be paid on a security.</skos:definition>
      <rdfs:subClassOf rdf:resource="&fibo-fnd-acc-dbt;DebtInterestPaymentTermsSet"/>
   </owl:Class>

   <owl:Class rdf:about="&fibo-sec-dbt-dbt-cfl;ExtendableMaturityRedemptionTermsSet">
      <rdfs:label>extendable maturity redemption terms set</rdfs:label>
      <skos:definition>Terms for the redemption of a security with extendable maturity.</skos:definition>
      <rdfs:subClassOf rdf:resource="&fibo-fnd-acc-dbt;DebtPrincipalRepaymentTermsSet"/>
   </owl:Class>

   <owl:Class rdf:about="&fibo-sec-dbt-dbt-cfl;FactorCalculationFormula">
      <rdfs:label>factor calculation formula</rdfs:label>
      <skos:definition>Formula for the determination of some variable factor which is then used in subsequent calculations. The result of such a formula is a parameter referred to by another formula.</skos:definition>
      <rdfs:subClassOf rdf:resource="&fibo-fnd-math-math;Formula"/>
   </owl:Class>

   <owl:Class rdf:about="&fibo-sec-dbt-dbt-cfl;InterestCalculationExpression">
      <rdfs:label>interest calculation expression</rdfs:label>
      <skos:definition>How the Formula is expressed i.e. the Right Hand Side of the Formula. This has separate parameters for Base and Margin. The overall Expression is not modeled but may be additionally described in a free form text field.</skos:definition>
      <rdfs:subClassOf rdf:resource="&fibo-fnd-math-math;FormulaExpression"/>
   </owl:Class>

   <owl:Class rdf:about="&fibo-sec-dbt-dbt-cfl;InterestCalculationFormula">
      <rdfs:label>interest calculation formula</rdfs:label>
      <skos:definition>Formula for calculation of Interest.</skos:definition>
   </owl:Class>

   <owl:Class rdf:about="&fibo-sec-dbt-dbt-cfl;InterestCalculationSubject">
      <rdfs:label>interest calculation subject</rdfs:label>
      <skos:definition>The Subject or Left Hand Side of an Interest Calculation Formula. This is by definition the Interest amount.</skos:definition>
      <rdfs:subClassOf rdf:resource="&fibo-fnd-math-math;FormulaSubject"/>
   </owl:Class>

   <owl:Class rdf:about="&fibo-sec-dbt-dbt-cfl;Margin">
      <rdfs:label>margin</rdfs:label>
      <skos:definition>The parameter of the Expression which is added to the Base to get the Interest amount.</skos:definition>
   </owl:Class>

   <owl:Class rdf:about="&fibo-sec-dbt-dbt-cfl;NonTradableDebtInterestTerms">
      <rdfs:label>non tradable debt interest terms</rdfs:label>
      <skos:definition>Terms for payment of interest on debt instruments that are not traded securities, i.e. over the counter, bilateral paper.</skos:definition>
   </owl:Class>

   <owl:Class rdf:about="&fibo-sec-dbt-dbt-cfl;PutSchedule">
      <rdfs:label>put schedule</rdfs:label>
   </owl:Class>

   <owl:Class rdf:about="&fibo-sec-dbt-dbt-cfl;PutScheduleListing">
      <rdfs:label>put schedule listing</rdfs:label>
      <skos:definition>Schedule of dates on which a Traded Security may be Put by the Holder.</skos:definition>
   </owl:Class>

   <owl:Class rdf:about="&fibo-sec-dbt-dbt-cfl;PutTermsSet">
      <rdfs:label>put terms set</rdfs:label>
      <skos:definition>Contractual terms for a feature that provides the bond holder the contractual option to redeem the bond prior to the scheduled maturity date.</skos:definition>
      <rdfs:subClassOf rdf:resource="&fibo-fnd-agr-ctr;ContractTermsSet"/>
   </owl:Class>

   <owl:Class rdf:about="&fibo-sec-dbt-dbt-cfl;PutWindow">
      <rdfs:label>put window</rdfs:label>
      <skos:definition>Window of number of days prior to a mandatory or optional redemption date that the issuer/agent must give notice to holders.</skos:definition>
   </owl:Class>

   <owl:Class rdf:about="&fibo-sec-dbt-dbt-cfl;RedemptionEvent">
      <rdfs:label>redemption event</rdfs:label>
      <skos:definition>An event whereby a debt security comes to the end of its life and the debt is paid off (redeemed).</skos:definition>
      <rdfs:subClassOf rdf:resource="&fibo-fnd-occ-evt;Event"/>
   </owl:Class>

   <owl:Class rdf:about="&fibo-sec-dbt-dbt-cfl;SecuritizedDebtInterest">
      <rdfs:label>securitized debt interest</rdfs:label>
      <skos:definition>Interest on Debt which is the subject of a Financial Security.</skos:definition>
      <rdfs:subClassOf rdf:resource="&fibo-fnd-acc-dbt;DebtInterest"/>
   </owl:Class>

   <owl:Class rdf:about="&fibo-sec-dbt-dbt-cfl;TradableDebtSecurityRedemptionTermsSet">
      <rdfs:label>tradable debt security redemption terms set</rdfs:label>
      <skos:definition>Terms for the redemption of the debt represented by a debt security.</skos:definition>
   </owl:Class>


  <!--
    ///////////////////////////////////////////////////////////////////////////////////////
    //
    // Individuals
    //
    ///////////////////////////////////////////////////////////////////////////////////////
    -->


</rdf:RDF>