<?xml version="1.0" encoding="UTF-8"?>
  
<!DOCTYPE rdf:RDF [
    <!ENTITY fibo-sec-dbt-dbt-par "http://spec.edmcouncil.org/fibo/red/sec/debt/debt-foundations/parity-variants/">
    <!ENTITY fibo-sec-dbt-dbt-ins "http://spec.edmcouncil.org/fibo/red/sec/debt/debt-foundations/debt-instruments/">
]>

<rdf:RDF xmlns:xsd="http://www.w3.org/2001/XMLSchema#"
         xmlns:sm="http://www.omg.org/techprocess/ab/SpecificationMetadata/"
         xmlns:xs="http://www.w3.org/2001/XMLSchema"
         xmlns:fibo-fnd-utl-av="http://www.omg.org/spec/EDMC-FIBO/FND/Utilities/AnnotationVocabulary/"
         xmlns:rdf="http://www.w3.org/1999/02/22-rdf-syntax-ns#"
         xmlns:rdfs="http://www.w3.org/2000/01/rdf-schema#"
         xmlns:owl="http://www.w3.org/2002/07/owl#"
         xmlns:skos="http://www.w3.org/2004/02/skos/core#"
         xmlns:dc="http://purl.org/dc/terms/"
         xml:base="http://spec.edmcouncil.org/fibo/red/sec/debt/debt-foundations/parity-variants/">

   <owl:Ontology rdf:about="http://spec.edmcouncil.org/fibo/red/sec/debt/debt-foundations/parity-variants/">
      <owl:imports rdf:resource="http://spec.edmcouncil.org/fibo/red/sec/debt/debt-foundations/debt-instruments/"/>
   </owl:Ontology>


  <!--
    ///////////////////////////////////////////////////////////////////////////////////////
    //
    // Datatypes
    //
    ///////////////////////////////////////////////////////////////////////////////////////
    -->


<rdfs:Datatype rdf:about="&fibo-sec-dbt-dbt-par;DebtRelativeValueSelection">
      <skos:definition>A relative value of a debt instrument at some point in time. This is exhaustively either par value, a discount or a premium.</skos:definition>
      <owl:equivalentClass>
         <rdfs:Datatype>
            <owl:oneOf>
               <rdf:Description>
                  <rdf:first rdf:datatype="http://www.w3.org/2001/XMLSchema#string">Discount</rdf:first>
                  <rdf:rest>
                     <rdf:Description>
                        <rdf:first rdf:datatype="http://www.w3.org/2001/XMLSchema#string">Premium</rdf:first>
                        <rdf:rest>
                           <rdf:Description>
                              <rdf:first rdf:datatype="http://www.w3.org/2001/XMLSchema#string">Par</rdf:first>
                              <rdf:rest rdf:resource="http://www.w3.org/1999/02/22-rdf-syntax-ns#nil"/>
                           </rdf:Description>
                        </rdf:rest>
                     </rdf:Description>
                  </rdf:rest>
               </rdf:Description>
            </owl:oneOf>
         </rdfs:Datatype>
      </owl:equivalentClass>
   </rdfs:Datatype>


  <!--
    ///////////////////////////////////////////////////////////////////////////////////////
    //
    // Object Properties
    //
    ///////////////////////////////////////////////////////////////////////////////////////
    -->



  <!--
    ///////////////////////////////////////////////////////////////////////////////////////
    //
    // Data Properties
    //
    ///////////////////////////////////////////////////////////////////////////////////////
    -->


<owl:DatatypeProperty rdf:about="&fibo-sec-dbt-dbt-par;valueAtIssue">
      <rdfs:label>value at issue</rdfs:label>
      <skos:definition>The relative value at which the instrument is issued, namely par, premium or discount. For Discount Instruments this is Discount.</skos:definition>
      <rdfs:range rdf:resource="&fibo-sec-dbt-dbt-par;DebtRelativeValueSelection"/>
   </owl:DatatypeProperty>

   <owl:DatatypeProperty rdf:about="&fibo-sec-dbt-dbt-par;valueAtIssue.1">
      <rdfs:label>value at issue</rdfs:label>
      <skos:definition>The relative value at which the instrument is issued, namely par, premium or discount. For Par Instrument this is defined as Par.</skos:definition>
      <rdfs:range rdf:resource="&fibo-sec-dbt-dbt-par;DebtRelativeValueSelection"/>
   </owl:DatatypeProperty>

   <owl:DatatypeProperty rdf:about="&fibo-sec-dbt-dbt-par;valueAtIssue.2">
      <rdfs:label>value at issue</rdfs:label>
      <skos:definition>The relative value at which the instrument is issued, namely par, premium or discount. For Premium Instrument this is Premium.</skos:definition>
      <rdfs:range rdf:resource="&fibo-sec-dbt-dbt-par;DebtRelativeValueSelection"/>
   </owl:DatatypeProperty>


  <!--
    ///////////////////////////////////////////////////////////////////////////////////////
    //
    // Annotation Properties
    //
    ///////////////////////////////////////////////////////////////////////////////////////
    -->



  <!--
    ///////////////////////////////////////////////////////////////////////////////////////
    //
    // Classes
    //
    ///////////////////////////////////////////////////////////////////////////////////////
    -->


<owl:Class rdf:about="&fibo-sec-dbt-dbt-par;DiscountedInstrument">
      <rdfs:label>discounted instrument</rdfs:label>
   </owl:Class>

   <owl:Class rdf:about="&fibo-sec-dbt-dbt-par;ParInstrument">
      <rdfs:label>par instrument</rdfs:label>
      <skos:definition>Instrument is issued at par. These instruments are issued at some face value and mature for a value equal to that face value plus interest.</skos:definition>
   </owl:Class>

   <owl:Class rdf:about="&fibo-sec-dbt-dbt-par;PremiumInstrument">
      <rdfs:label>premium instrument</rdfs:label>
   </owl:Class>


  <!--
    ///////////////////////////////////////////////////////////////////////////////////////
    //
    // Individuals
    //
    ///////////////////////////////////////////////////////////////////////////////////////
    -->


</rdf:RDF>