<?xml version="1.0" encoding="UTF-8"?>
  
<!DOCTYPE rdf:RDF [
    <!ENTITY fibo-sec-dbt-mm-tr "http://spec.edmcouncil.org/fibo/red/sec/debt/money-markets/traded-short-term-debt/">
    <!ENTITY fibo-fnd-acc-acc "http://spec.edmcouncil.org/fibo/red/fnd/accounting/accounting-main/">
    <!ENTITY fibo-fnd-acc-dbt "http://spec.edmcouncil.org/fibo/red/fnd/accounting/debt-terms/">
    <!ENTITY fibo-fnd-tim-tim "http://spec.edmcouncil.org/fibo/red/fnd/date-time/date-time/">
    <!ENTITY fibo-sec-sec-iss "http://spec.edmcouncil.org/fibo/red/sec/securities/securities-issuance-terms/">
    <!ENTITY fibo-sec-dbt-dbt-ins "http://spec.edmcouncil.org/fibo/red/sec/debt/debt-foundations/debt-instruments/">
    <!ENTITY fibo-be-fct-se "http://spec.edmcouncil.org/fibo/red/be/functional-entities-ext/state-entities/">
    <!ENTITY fibo-fnd-agr-ctr "http://spec.edmcouncil.org/fibo/red/fnd/agreements/contracts/">
    <!ENTITY fibo-sec-dbt-mm-repo "http://spec.edmcouncil.org/fibo/red/sec/debt/money-markets/repo/">
    <!ENTITY fibo-fnd-utl-bt "http://spec.edmcouncil.org/fibo/red/fnd/utilities/business-facing-types/">
    <!ENTITY fibo-sec-dbt-dbt-cfl "http://spec.edmcouncil.org/fibo/red/sec/debt/debt-foundations/debt-cashflow-terms/">
    <!ENTITY fibo-sec-dbt-dbt-par "http://spec.edmcouncil.org/fibo/red/sec/debt/debt-foundations/parity-variants/">
    <!ENTITY fibo-sec-dbt-bond-iss "http://spec.edmcouncil.org/fibo/red/sec/debt/bonds/bonds-issuer-variants/">
    <!ENTITY fibo-be-le-fbo "http://spec.edmcouncil.org/fibo/red/be/legal-entities/formal-business-organizations/">
]>

<rdf:RDF xmlns:xsd="http://www.w3.org/2001/XMLSchema#"
         xmlns:sm="http://www.omg.org/techprocess/ab/SpecificationMetadata/"
         xmlns:xs="http://www.w3.org/2001/XMLSchema"
         xmlns:fibo-fnd-utl-av="http://www.omg.org/spec/EDMC-FIBO/FND/Utilities/AnnotationVocabulary/"
         xmlns:rdf="http://www.w3.org/1999/02/22-rdf-syntax-ns#"
         xmlns:rdfs="http://www.w3.org/2000/01/rdf-schema#"
         xmlns:owl="http://www.w3.org/2002/07/owl#"
         xmlns:skos="http://www.w3.org/2004/02/skos/core#"
         xmlns:dc="http://purl.org/dc/terms/"
         xml:base="http://spec.edmcouncil.org/fibo/red/sec/debt/money-markets/traded-short-term-debt/">

   <owl:Ontology rdf:about="http://spec.edmcouncil.org/fibo/red/sec/debt/money-markets/traded-short-term-debt/">
      <owl:imports rdf:resource="http://spec.edmcouncil.org/fibo/red/fnd/accounting/accounting-main/"/>
      <owl:imports rdf:resource="http://spec.edmcouncil.org/fibo/red/fnd/accounting/debt-terms/"/>
      <owl:imports rdf:resource="http://spec.edmcouncil.org/fibo/red/fnd/date-time/date-time/"/>
      <owl:imports rdf:resource="http://spec.edmcouncil.org/fibo/red/sec/securities/securities-issuance-terms/"/>
      <owl:imports rdf:resource="http://spec.edmcouncil.org/fibo/red/sec/debt/debt-foundations/debt-instruments/"/>
      <owl:imports rdf:resource="http://spec.edmcouncil.org/fibo/red/be/functional-entities-ext/state-entities/"/>
      <owl:imports rdf:resource="http://spec.edmcouncil.org/fibo/red/fnd/agreements/contracts/"/>
      <owl:imports rdf:resource="http://spec.edmcouncil.org/fibo/red/sec/debt/money-markets/repo/"/>
      <owl:imports rdf:resource="http://spec.edmcouncil.org/fibo/red/fnd/utilities/business-facing-types/"/>
      <owl:imports rdf:resource="http://spec.edmcouncil.org/fibo/red/sec/debt/debt-foundations/debt-cashflow-terms/"/>
      <owl:imports rdf:resource="http://spec.edmcouncil.org/fibo/red/sec/debt/debt-foundations/parity-variants/"/>
      <owl:imports rdf:resource="http://spec.edmcouncil.org/fibo/red/sec/debt/bonds/bonds-issuer-variants/"/>
      <owl:imports rdf:resource="http://spec.edmcouncil.org/fibo/red/be/legal-entities/formal-business-organizations/"/>
   </owl:Ontology>


  <!--
    ///////////////////////////////////////////////////////////////////////////////////////
    //
    // Datatypes
    //
    ///////////////////////////////////////////////////////////////////////////////////////
    -->



  <!--
    ///////////////////////////////////////////////////////////////////////////////////////
    //
    // Object Properties
    //
    ///////////////////////////////////////////////////////////////////////////////////////
    -->


<owl:ObjectProperty rdf:about="&fibo-sec-dbt-mm-tr;identifiedAs">
      <rdfs:label>identified as</rdfs:label>
      <rdfs:subPropertyOf rdf:resource="&fibo-sec-sec-iss;identity"/>
      <rdfs:domain rdf:resource="&fibo-sec-dbt-mm-tr;CommercialPaperIssuer"/>
      <rdfs:range rdf:resource="&fibo-sec-dbt-mm-tr;.UnionClass.4"/>
   </owl:ObjectProperty>

   <owl:ObjectProperty rdf:about="&fibo-sec-dbt-mm-tr;issuer">
      <rdfs:label>issuer</rdfs:label>
      <rdfs:subPropertyOf rdf:resource="&fibo-sec-sec-iss;issuer"/>
      <rdfs:domain rdf:resource="&fibo-sec-dbt-mm-tr;CommercialPaper"/>
      <rdfs:range rdf:resource="&fibo-sec-dbt-mm-tr;CommercialPaperIssuer"/>
   </owl:ObjectProperty>

   <owl:ObjectProperty rdf:about="&fibo-sec-dbt-mm-tr;hasMaturityDuration">
      <rdfs:label>has maturity duration</rdfs:label>
      <rdfs:domain rdf:resource="&fibo-sec-dbt-mm-tr;CommercialPaper"/>
      <rdfs:range rdf:resource="&fibo-fnd-tim-tim;TypicalDuration"/>
   </owl:ObjectProperty>

   <owl:ObjectProperty rdf:about="&fibo-sec-dbt-mm-tr;valueAtMaturity.4">
      <rdfs:label>value at maturity</rdfs:label>
      <skos:definition>The value at which the instrument matures, namely par, discount or premium. These instruments mature at par and pay interest.</skos:definition>
      <rdfs:domain rdf:resource="&fibo-sec-dbt-mm-tr;InterestBearingCP"/>
      <rdfs:range rdf:resource="&fibo-sec-dbt-dbt-par;DebtRelativeValueSelection"/>
   </owl:ObjectProperty>

   <owl:ObjectProperty rdf:about="&fibo-sec-dbt-mm-tr;typicalMaturityDuration">
      <rdfs:label>typical maturity duration</rdfs:label>
      <rdfs:domain rdf:resource="&fibo-sec-dbt-mm-tr;.UnionClass.68"/>
      <rdfs:range rdf:resource="&fibo-fnd-tim-tim;UpToOneYear"/>
   </owl:ObjectProperty>

   <owl:ObjectProperty rdf:about="&fibo-sec-dbt-mm-tr;hasInterestPaymentTerms">
      <rdfs:label>has interest payment terms</rdfs:label>
      <rdfs:subPropertyOf rdf:resource="&fibo-fnd-agr-ctr;contractHasTerms"/>
      <rdfs:domain rdf:resource="&fibo-sec-dbt-dbt-ins;NonTradableDebtInstrument"/>
      <rdfs:range rdf:resource="&fibo-sec-dbt-dbt-cfl;NonTradableDebtInterestTerms"/>
   </owl:ObjectProperty>

   <owl:ObjectProperty rdf:about="&fibo-sec-dbt-mm-tr;issuer.1">
      <rdfs:label>issuer</rdfs:label>
      <rdfs:subPropertyOf rdf:resource="&fibo-sec-sec-iss;issuer"/>
      <rdfs:domain rdf:resource="&fibo-sec-dbt-mm-tr;TreasuryBill"/>
      <rdfs:range rdf:resource="&fibo-sec-dbt-bond-iss;GovernmentDebtIssuer"/>
   </owl:ObjectProperty>

   <owl:ObjectProperty rdf:about="&fibo-sec-dbt-mm-tr;maturityDuration">
      <rdfs:label>maturity duration</rdfs:label>
      <rdfs:domain rdf:resource="&fibo-sec-dbt-mm-tr;TermCertificateOfDeposit"/>
      <rdfs:range rdf:resource="&fibo-fnd-tim-tim;DurationOfMoreThanOneYear"/>
   </owl:ObjectProperty>


  <!--
    ///////////////////////////////////////////////////////////////////////////////////////
    //
    // Data Properties
    //
    ///////////////////////////////////////////////////////////////////////////////////////
    -->


<owl:DatatypeProperty rdf:about="&fibo-sec-dbt-mm-tr;callable">
      <rdfs:label>callable</rdfs:label>
      <skos:definition>Whether the issuer of the debt instrument can call the debt prior to maturity. This instrument is not callable.</skos:definition>
      <rdfs:range rdf:resource="&fibo-fnd-utl-bt;yesOrNo"/>
   </owl:DatatypeProperty>

   <owl:DatatypeProperty rdf:about="&fibo-sec-dbt-mm-tr;putable">
      <rdfs:label>putable</rdfs:label>
      <skos:definition>Whether the holder has the right to ask for redemption of the security prior to final maturity. This instrument is not putable.</skos:definition>
      <rdfs:range rdf:resource="&fibo-fnd-utl-bt;yesOrNo"/>
   </owl:DatatypeProperty>

   <owl:DatatypeProperty rdf:about="&fibo-sec-dbt-mm-tr;strippable">
      <rdfs:label>strippable</rdfs:label>
      <skos:definition>Whether or not the instrument can be stripped, so that interest and principal may be traded separately. This instrument cannot be stripped.</skos:definition>
      <rdfs:range rdf:resource="&fibo-fnd-utl-bt;yesOrNo"/>
   </owl:DatatypeProperty>

   <owl:DatatypeProperty rdf:about="&fibo-sec-dbt-mm-tr;valueAtIssue">
      <rdfs:label>value at issue</rdfs:label>
      <skos:definition>The relative value at which the instrument is issued, namely par, premium or discount. These instruments are issued at a discount.</skos:definition>
      <rdfs:range rdf:resource="&fibo-sec-dbt-dbt-par;DebtRelativeValueSelection"/>
   </owl:DatatypeProperty>

   <owl:DatatypeProperty rdf:about="&fibo-sec-dbt-mm-tr;valueAtMaturity">
      <rdfs:label>value at maturity</rdfs:label>
      <skos:definition>The value at which the instrument matures, namely par, discount or premium. These instruments mature at par.</skos:definition>
      <rdfs:range rdf:resource="&fibo-sec-dbt-dbt-par;DebtRelativeValueSelection"/>
   </owl:DatatypeProperty>

   <owl:DatatypeProperty rdf:about="&fibo-sec-dbt-mm-tr;multiplier">
      <rdfs:label>multiplier</rdfs:label>
      <skos:definition>The typical duration for the CP instrument.</skos:definition>
      <rdfs:range rdf:resource="&fibo-fnd-utl-bt;wholeNumber"/>
   </owl:DatatypeProperty>

   <owl:DatatypeProperty rdf:about="&fibo-sec-dbt-mm-tr;callable.1">
      <rdfs:label>callable</rdfs:label>
      <skos:definition>Whether the issuer of the debt instrument can call the debt prior to maturity. This instrument is not callable.</skos:definition>
      <rdfs:range rdf:resource="&fibo-fnd-utl-bt;yesOrNo"/>
   </owl:DatatypeProperty>

   <owl:DatatypeProperty rdf:about="&fibo-sec-dbt-mm-tr;putable.1">
      <rdfs:label>putable</rdfs:label>
      <skos:definition>Whether the holder has the right to ask for redemption of the security prior to final maturity. This instrument is not putable.</skos:definition>
      <rdfs:range rdf:resource="&fibo-fnd-utl-bt;yesOrNo"/>
   </owl:DatatypeProperty>

   <owl:DatatypeProperty rdf:about="&fibo-sec-dbt-mm-tr;strippable.1">
      <rdfs:label>strippable</rdfs:label>
      <skos:definition>Whether or not the instrument can be stripped, so that interest and principal may be traded separately. This instrument cannot be stripped.</skos:definition>
      <rdfs:range rdf:resource="&fibo-fnd-utl-bt;yesOrNo"/>
   </owl:DatatypeProperty>

   <owl:DatatypeProperty rdf:about="&fibo-sec-dbt-mm-tr;valueAtIssue.1">
      <rdfs:label>value at issue</rdfs:label>
      <skos:definition>The relative value at which the instrument is issued, namely par, premium or discount. These instruments are issued at par.</skos:definition>
      <rdfs:range rdf:resource="&fibo-sec-dbt-dbt-par;DebtRelativeValueSelection"/>
   </owl:DatatypeProperty>

   <owl:DatatypeProperty rdf:about="&fibo-sec-dbt-mm-tr;valueAtMaturity.1">
      <rdfs:label>value at maturity</rdfs:label>
      <skos:definition>The value at which the instrument matures, namely par, discount or premium. These instruments mature at par with interest.</skos:definition>
      <rdfs:range rdf:resource="&fibo-sec-dbt-dbt-par;DebtRelativeValueSelection"/>
   </owl:DatatypeProperty>

   <owl:DatatypeProperty rdf:about="&fibo-sec-dbt-mm-tr;callable.2">
      <rdfs:label>callable</rdfs:label>
      <skos:definition>Whether the issuer of the debt instrument can call the debt prior to maturity. This instrument is not callable.</skos:definition>
      <rdfs:range rdf:resource="&fibo-fnd-utl-bt;yesOrNo"/>
   </owl:DatatypeProperty>

   <owl:DatatypeProperty rdf:about="&fibo-sec-dbt-mm-tr;putable.2">
      <rdfs:label>putable</rdfs:label>
      <skos:definition>Whether the holder has the right to ask for redemption of the security prior to final maturity. This instrument is not putable.</skos:definition>
      <rdfs:range rdf:resource="&fibo-fnd-utl-bt;yesOrNo"/>
   </owl:DatatypeProperty>

   <owl:DatatypeProperty rdf:about="&fibo-sec-dbt-mm-tr;strippable.2">
      <rdfs:label>strippable</rdfs:label>
      <skos:definition>Whether or not the instrument can be stripped, so that interest and principal may be traded separately. This instrument cannot be stripped.</skos:definition>
      <rdfs:range rdf:resource="&fibo-fnd-utl-bt;yesOrNo"/>
   </owl:DatatypeProperty>

   <owl:DatatypeProperty rdf:about="&fibo-sec-dbt-mm-tr;valueAtMaturity.2">
      <rdfs:label>value at maturity</rdfs:label>
      <skos:definition>The value at which the instrument matures, namely par, discount or premium. These instruments mature at par.</skos:definition>
      <rdfs:range rdf:resource="&fibo-sec-dbt-dbt-par;DebtRelativeValueSelection"/>
   </owl:DatatypeProperty>

   <owl:DatatypeProperty rdf:about="&fibo-sec-dbt-mm-tr;valueAtIssue.2">
      <rdfs:label>value at issue</rdfs:label>
      <skos:definition>The relative value at which the instrument is issued, namely par, premium or discount. These instruments are issued at a discount.</skos:definition>
      <rdfs:range rdf:resource="&fibo-sec-dbt-dbt-par;DebtRelativeValueSelection"/>
   </owl:DatatypeProperty>

   <owl:DatatypeProperty rdf:about="&fibo-sec-dbt-mm-tr;valueAtMaturity.3">
      <rdfs:label>value at maturity</rdfs:label>
      <skos:definition>The value at which the instrument matures, namely par, discount or premium. These instruments mature at par.</skos:definition>
      <rdfs:range rdf:resource="&fibo-sec-dbt-dbt-par;DebtRelativeValueSelection"/>
   </owl:DatatypeProperty>

   <owl:DatatypeProperty rdf:about="&fibo-sec-dbt-mm-tr;valueAtIssue.3">
      <rdfs:label>value at issue</rdfs:label>
      <skos:definition>The relative value at which the instrument is issued, namely par, premium or discount. These instruments are issued at par.</skos:definition>
      <rdfs:range rdf:resource="&fibo-sec-dbt-dbt-par;DebtRelativeValueSelection"/>
   </owl:DatatypeProperty>

   <owl:DatatypeProperty rdf:about="&fibo-sec-dbt-mm-tr;callable.3">
      <rdfs:label>callable</rdfs:label>
      <skos:definition>Whether the writer of the debt contract (the debtor) can call the debt prior to maturity. This instrument is not callable.</skos:definition>
      <rdfs:range rdf:resource="&fibo-fnd-utl-bt;yesOrNo"/>
   </owl:DatatypeProperty>

   <owl:DatatypeProperty rdf:about="&fibo-sec-dbt-mm-tr;putable.3">
      <rdfs:label>putable</rdfs:label>
      <skos:definition>Whether the holder has the right to ask for redemption of the security prior to final maturity. This instrument is not putable.</skos:definition>
      <rdfs:range rdf:resource="&fibo-fnd-utl-bt;yesOrNo"/>
   </owl:DatatypeProperty>

   <owl:DatatypeProperty rdf:about="&fibo-sec-dbt-mm-tr;valueAtIssue.4">
      <rdfs:label>value at issue</rdfs:label>
      <skos:definition>The relative value at which the instrument is issued, namely par, premium or discount. These instruments are issued at par.</skos:definition>
      <rdfs:range rdf:resource="&fibo-sec-dbt-dbt-par;DebtRelativeValueSelection"/>
   </owl:DatatypeProperty>

   <owl:DatatypeProperty rdf:about="&fibo-sec-dbt-mm-tr;valueAtMaturity.5">
      <rdfs:label>value at maturity</rdfs:label>
      <skos:definition>The value at which the instrument matures, namely par, discount or premium. These instruments mature at par.</skos:definition>
      <rdfs:range rdf:resource="&fibo-sec-dbt-dbt-par;DebtRelativeValueSelection"/>
   </owl:DatatypeProperty>

   <owl:DatatypeProperty rdf:about="&fibo-sec-dbt-mm-tr;maturityDate">
      <rdfs:label>maturity date</rdfs:label>
      <skos:definition>The date when the debt is scheduled to be repaid.</skos:definition>
      <rdfs:range rdf:resource="http://www.w3.org/2001/XMLSchema#date"/>
   </owl:DatatypeProperty>

   <owl:DatatypeProperty rdf:about="&fibo-sec-dbt-mm-tr;callable.4">
      <rdfs:label>callable</rdfs:label>
      <skos:definition>Whether the issuer of the debt instrument can call the debt prior to maturity. This instrument is not callable.</skos:definition>
      <rdfs:range rdf:resource="&fibo-fnd-utl-bt;yesOrNo"/>
   </owl:DatatypeProperty>

   <owl:DatatypeProperty rdf:about="&fibo-sec-dbt-mm-tr;putable.4">
      <rdfs:label>putable</rdfs:label>
      <skos:definition>Whether the holder has the right to ask for redemption of the security prior to final maturity. This instrument is not putable.</skos:definition>
      <rdfs:range rdf:resource="&fibo-fnd-utl-bt;yesOrNo"/>
   </owl:DatatypeProperty>

   <owl:DatatypeProperty rdf:about="&fibo-sec-dbt-mm-tr;strippable.3">
      <rdfs:label>strippable</rdfs:label>
      <skos:definition>Whether or not the instrument can be stripped, so that interest and principal may be traded separately. This instrument cannot be stripped.</skos:definition>
      <rdfs:range rdf:resource="&fibo-fnd-utl-bt;yesOrNo"/>
   </owl:DatatypeProperty>

   <owl:DatatypeProperty rdf:about="&fibo-sec-dbt-mm-tr;valueAtIssue.5">
      <rdfs:label>value at issue</rdfs:label>
      <skos:definition>The relative value at which the instrument is issued, namely par, premium or discount. These instruments are issued at a discount.</skos:definition>
      <rdfs:range rdf:resource="&fibo-sec-dbt-dbt-par;DebtRelativeValueSelection"/>
   </owl:DatatypeProperty>

   <owl:DatatypeProperty rdf:about="&fibo-sec-dbt-mm-tr;valueAtMaturity.6">
      <rdfs:label>value at maturity</rdfs:label>
      <skos:definition>The value at which the instrument matures, namely par, discount or premium. These instruments mature at par.</skos:definition>
      <rdfs:range rdf:resource="&fibo-sec-dbt-dbt-par;DebtRelativeValueSelection"/>
   </owl:DatatypeProperty>


  <!--
    ///////////////////////////////////////////////////////////////////////////////////////
    //
    // Annotation Properties
    //
    ///////////////////////////////////////////////////////////////////////////////////////
    -->



  <!--
    ///////////////////////////////////////////////////////////////////////////////////////
    //
    // Classes
    //
    ///////////////////////////////////////////////////////////////////////////////////////
    -->


<owl:Class rdf:about="&fibo-sec-dbt-mm-tr;.UnionClass.4">
      <skos:definition>An entity which is an Organization or some kind of Government such as a Municipal Government.</skos:definition>
      <owl:equivalentClass>
         <owl:Class>
            <owl:unionOf rdf:parseType="Collection">
               <owl:Class rdf:about="&fibo-be-le-fbo;FormallyConstitutedOrganization"/>
               <owl:Class rdf:about="&fibo-be-fct-se;Government"/>
            </owl:unionOf>
         </owl:Class>
      </owl:equivalentClass>
   </owl:Class>

   <owl:Class rdf:about="&fibo-sec-dbt-mm-tr;BankersAcceptance">
      <rdfs:label>bankers acceptance</rdfs:label>
      <skos:definition>A Draft where the drawer and drawee of the draft are distinct parties and the drawee is a bank.</skos:definition>
      <rdfs:subClassOf rdf:resource="&fibo-sec-dbt-dbt-ins;TradableDebtInstrument"/>
      <rdfs:subClassOf rdf:resource="&fibo-fnd-acc-acc;Draft"/>
   </owl:Class>

   <owl:Class rdf:about="&fibo-sec-dbt-mm-tr;BillOfExchange">
      <rdfs:label>bill of exchange</rdfs:label>
   </owl:Class>

   <owl:Class rdf:about="&fibo-sec-dbt-mm-tr;CPTypicalDurationDescription">
      <rdfs:label>c p typical duration description</rdfs:label>
      <skos:definition>The formal description of the typical period of time which is the mayturity of a Commercial Paper instrument.</skos:definition>
      <rdfs:subClassOf rdf:resource="&fibo-fnd-tim-tim;DurationDescription"/>
   </owl:Class>

   <owl:Class rdf:about="&fibo-sec-dbt-mm-tr;CertificateOfDeposit">
      <rdfs:label>certificate of deposit</rdfs:label>
      <skos:definition>A certificate of deposit (CD) is a money market instrument issued by a depository institution as evidence of a time deposit.</skos:definition>
   </owl:Class>

   <owl:Class rdf:about="&fibo-sec-dbt-mm-tr;CommercialPaper">
      <rdfs:label>commercial paper</rdfs:label>
      <skos:definition>Commercial paper (CP) is unsecured short-term promissory notes issued primarily by corporations, although there are also municipal and sovereign issuers (not included in this definition).</skos:definition>
   </owl:Class>

   <owl:Class rdf:about="&fibo-sec-dbt-mm-tr;CommercialPaperIssuer">
      <rdfs:label>commercial paper issuer</rdfs:label>
      <skos:definition>Any entity that issues Commercial Paper. This includes corporations but the Special Purpose Entities that issue Asset Backed Commercial Paper (ABCP) and some mutual funds also issue CP. Can also be a banks, an institution, pretty much anything. There are no hard and fast criteria for this. Therefore this is defined as being any kind of Organization or any kind of Government.</skos:definition>
      <rdfs:subClassOf rdf:resource="&fibo-sec-sec-iss;SecurityIssuer"/>
   </owl:Class>

   <owl:Class rdf:about="&fibo-sec-dbt-mm-tr;DiscountedCP">
      <rdfs:label>discounted c p</rdfs:label>
      <skos:definition>A Discounted CP is similar to a Treasury Bill except the maturity is 270 days or less. Therefore (draft definition): A Money Market instrument (short term debt instrument) issued by a corporation for the purposes of raising funds. This is tradable and accretes interest i.e. it is a Discounted Instrument. It has a maturity of 270 days or less.</skos:definition>
      <rdfs:subClassOf rdf:resource="&fibo-sec-dbt-mm-tr;CommercialPaper"/>
   </owl:Class>

   <owl:Class rdf:about="&fibo-sec-dbt-mm-tr;EurodollarDeposit">
      <rdfs:label>eurodollar deposit</rdfs:label>
      <skos:definition>A US dollar deposit or other currency deposit made outside the US or the country that issues that currency. Further notes from riskglossary.com (part of Money Market Deposit article): The Eurodollar market has become global, so its name is a bit of a misnomer. A bank in Japan or Singapore may accept dollar deposits, but these are still called Eurodollar deposits. The market also includes other currencies, so there are Eurosterling, Euroyen, Euroswiss, etc. To confuse matters, in 1999, the European Union embraced the euro as its new currency, so you can now hear of Euroeuro. Eurocurrency is the general term for any currency deposited in bank branches outside countries where it is the national currency. Comment: Should this not rather be labeled as Eurocurrency Deposit, corresponding with the above definition? Eurodollar deposit would be a dollar-denominated sub type of this.</skos:definition>
      <rdfs:subClassOf rdf:resource="&fibo-sec-dbt-mm-tr;MoneyMarketDeposit"/>
   </owl:Class>

   <owl:Class rdf:about="&fibo-sec-dbt-mm-tr;InterestBearingCP">
      <rdfs:label>interest bearing c p</rdfs:label>
      <skos:definition>Interest Bearing Commercial Paper is sold at par and has interest rate but only pays interest at maturity.</skos:definition>
   </owl:Class>

   <owl:Class rdf:about="&fibo-sec-dbt-mm-tr;MoneyMarketDeposit">
      <rdfs:label>money market deposit</rdfs:label>
      <rdfs:subClassOf rdf:resource="&fibo-sec-dbt-dbt-ins;NonTradableDebtInstrument"/>
   </owl:Class>

   <owl:Class rdf:about="&fibo-sec-dbt-mm-tr;NonTradableDebtRedemptionTerms">
      <rdfs:label>non tradable debt redemption terms</rdfs:label>
      <skos:definition>Terms for repayment of principal on debt instruments that are not traded securities, i.e. over the counter, bilateral paper.</skos:definition>
      <rdfs:subClassOf rdf:resource="&fibo-fnd-acc-dbt;DebtPrincipalRepaymentTermsSet"/>
   </owl:Class>

   <owl:Class rdf:about="&fibo-sec-dbt-mm-tr;TermCertificateOfDeposit">
      <rdfs:label>term certificate of deposit</rdfs:label>
      <skos:definition>A Certificate of Deposit with a maturity duration of more than one year.</skos:definition>
      <rdfs:subClassOf rdf:resource="&fibo-sec-dbt-mm-tr;CertificateOfDeposit"/>
   </owl:Class>

   <owl:Class rdf:about="&fibo-sec-dbt-mm-tr;TreasuryBill">
      <rdfs:label>treasury bill</rdfs:label>
   </owl:Class>

   <owl:Class rdf:about="&fibo-sec-dbt-mm-tr;.UnionClass.68">
      <skos:definition>Money Market Debt Instrument is a kind of short term debt security. This is defined as the logical union of all the securities that are commonly referred to as Money Market instruments.</skos:definition>
      <owl:equivalentClass>
         <owl:Class>
            <owl:unionOf rdf:parseType="Collection">
               <owl:Class rdf:about="&fibo-sec-dbt-mm-repo;RepurchaseAgreement"/>
               <owl:Class rdf:about="&fibo-sec-dbt-mm-tr;BankersAcceptance"/>
               <owl:Class rdf:about="&fibo-sec-dbt-mm-tr;TreasuryBill"/>
               <owl:Class rdf:about="&fibo-sec-dbt-mm-tr;CommercialPaper"/>
               <owl:Class rdf:about="&fibo-sec-dbt-mm-tr;MoneyMarketDeposit"/>
               <owl:Class rdf:about="&fibo-sec-dbt-mm-tr;CertificateOfDeposit"/>
            </owl:unionOf>
         </owl:Class>
      </owl:equivalentClass>
   </owl:Class>


  <!--
    ///////////////////////////////////////////////////////////////////////////////////////
    //
    // Individuals
    //
    ///////////////////////////////////////////////////////////////////////////////////////
    -->


</rdf:RDF>