<?xml version="1.0" encoding="UTF-8"?>
  
<!DOCTYPE rdf:RDF [
    <!ENTITY fibo-ind-fx-fx "http://spec.edmcouncil.org/fibo/red/ind/foreign-exchange/foreign-exchange/">
    <!ENTITY fibo-ind-ind-ind "http://spec.edmcouncil.org/fibo/red/ind/indicators/indicators/">
    <!ENTITY fibo-ind-ind-val "http://spec.edmcouncil.org/fibo/red/ind/indicators/indicators-values/">
    <!ENTITY fibo-fnd-acc-cur "http://spec.edmcouncil.org/fibo/red/fnd/accounting/currency-amount/">
    <!ENTITY fibo-fnd-tim-tim "http://spec.edmcouncil.org/fibo/red/fnd/date-time/date-time/">
]>

<rdf:RDF xmlns:xsd="http://www.w3.org/2001/XMLSchema#"
         xmlns:sm="http://www.omg.org/techprocess/ab/SpecificationMetadata/"
         xmlns:xs="http://www.w3.org/2001/XMLSchema"
         xmlns:fibo-fnd-utl-av="http://www.omg.org/spec/EDMC-FIBO/FND/Utilities/AnnotationVocabulary/"
         xmlns:rdf="http://www.w3.org/1999/02/22-rdf-syntax-ns#"
         xmlns:rdfs="http://www.w3.org/2000/01/rdf-schema#"
         xmlns:owl="http://www.w3.org/2002/07/owl#"
         xmlns:skos="http://www.w3.org/2004/02/skos/core#"
         xmlns:dc="http://purl.org/dc/terms/"
         xml:base="http://spec.edmcouncil.org/fibo/red/ind/foreign-exchange/foreign-exchange/">

   <owl:Ontology rdf:about="http://spec.edmcouncil.org/fibo/red/ind/foreign-exchange/foreign-exchange/">
      <owl:imports rdf:resource="http://spec.edmcouncil.org/fibo/red/ind/indicators/indicators/"/>
      <owl:imports rdf:resource="http://spec.edmcouncil.org/fibo/red/ind/indicators/indicators-values/"/>
      <owl:imports rdf:resource="http://spec.edmcouncil.org/fibo/red/fnd/accounting/currency-amount/"/>
      <owl:imports rdf:resource="http://spec.edmcouncil.org/fibo/red/fnd/date-time/date-time/"/>
   </owl:Ontology>


  <!--
    ///////////////////////////////////////////////////////////////////////////////////////
    //
    // Datatypes
    //
    ///////////////////////////////////////////////////////////////////////////////////////
    -->



  <!--
    ///////////////////////////////////////////////////////////////////////////////////////
    //
    // Object Properties
    //
    ///////////////////////////////////////////////////////////////////////////////////////
    -->


<owl:ObjectProperty rdf:about="&fibo-ind-fx-fx;hasNumericValue">
      <rdfs:label>has numeric value</rdfs:label>
      <skos:definition>The actual value of the exchange rate, stated as a number which is the price paid for the denominator currency in units of the numerator currency.</skos:definition>
      <rdfs:domain rdf:resource="&fibo-ind-fx-fx;ExchangeRate"/>
      <rdfs:range rdf:resource="&fibo-ind-ind-val;ExchangeRateTimedValue"/>
   </owl:ObjectProperty>

   <owl:ObjectProperty rdf:about="&fibo-ind-fx-fx;hasBaseCurrency">
      <rdfs:label>has base currency</rdfs:label>
      <skos:definition>The currency used as the denominator of the exchange rate. One unit of this currency represents R units of the dealt currency, where R is the Exchange Rate value.</skos:definition>
      <rdfs:domain rdf:resource="&fibo-ind-fx-fx;ExchangeRate"/>
      <rdfs:range rdf:resource="&fibo-fnd-acc-cur;Currency"/>
   </owl:ObjectProperty>

   <owl:ObjectProperty rdf:about="&fibo-ind-fx-fx;hasDealtCurrency">
      <rdfs:label>has dealt currency</rdfs:label>
      <skos:definition>The currency used as the numerator of the exchange rate. R units of this currency represent one unit of the base currency.</skos:definition>
      <rdfs:domain rdf:resource="&fibo-ind-fx-fx;ExchangeRate"/>
      <rdfs:range rdf:resource="&fibo-fnd-acc-cur;Currency"/>
   </owl:ObjectProperty>

   <owl:ObjectProperty rdf:about="&fibo-ind-fx-fx;fXSpotVolatilityIsVolatilityOf">
      <rdfs:label>f x spot volatility is volatility of</rdfs:label>
      <skos:definition>The currency spot rate to which the volatility measure applies and of which it is a measure.</skos:definition>
      <rdfs:subPropertyOf rdf:resource="&fibo-ind-ind-ind;isVolatilityOf"/>
      <rdfs:domain rdf:resource="&fibo-ind-fx-fx;FXSpotVolatility"/>
      <rdfs:range rdf:resource="&fibo-ind-fx-fx;CurrencySpotRate"/>
   </owl:ObjectProperty>


  <!--
    ///////////////////////////////////////////////////////////////////////////////////////
    //
    // Data Properties
    //
    ///////////////////////////////////////////////////////////////////////////////////////
    -->


<owl:DatatypeProperty rdf:about="&fibo-ind-fx-fx;hasSettlementDate">
      <rdfs:label>has settlement date</rdfs:label>
      <skos:definition>The date for forward settlement of currency transactions at this forward exchange rate.</skos:definition>
      <rdfs:range rdf:resource="&fibo-fnd-tim-tim;Date"/>
   </owl:DatatypeProperty>


  <!--
    ///////////////////////////////////////////////////////////////////////////////////////
    //
    // Annotation Properties
    //
    ///////////////////////////////////////////////////////////////////////////////////////
    -->



  <!--
    ///////////////////////////////////////////////////////////////////////////////////////
    //
    // Classes
    //
    ///////////////////////////////////////////////////////////////////////////////////////
    -->


<owl:Class rdf:about="&fibo-ind-fx-fx;CurrencyForwardRate">
      <rdfs:label>currency forward rate</rdfs:label>
      <rdfs:subClassOf rdf:resource="&fibo-ind-fx-fx;ExchangeRate"/>
   </owl:Class>

   <owl:Class rdf:about="&fibo-ind-fx-fx;CurrencySpotRate">
      <rdfs:label>currency spot rate</rdfs:label>
      <skos:definition>The exchange rate at a point in time, with settlement at that same point in time.</skos:definition>
   </owl:Class>

   <owl:Class rdf:about="&fibo-ind-fx-fx;ExchangeRate">
      <rdfs:label>exchange rate</rdfs:label>
      <rdfs:subClassOf rdf:resource="&fibo-ind-ind-ind;MarketBaseRate"/>
   </owl:Class>

   <owl:Class rdf:about="&fibo-ind-fx-fx;FXSpotVolatility">
      <rdfs:label>f x spot volatility</rdfs:label>
      <skos:definition>A measure of exchange rate fluctuation. Mathematically the volatility is the annualized standard deviation of the daily changes in the exchange rate. Definition Adapted From: OptionsEducation.org adapted (replaced "stock" with "Exchange Rate" and re-phrased)</skos:definition>
      <rdfs:subClassOf rdf:resource="&fibo-ind-ind-ind;Volatility"/>
   </owl:Class>


  <!--
    ///////////////////////////////////////////////////////////////////////////////////////
    //
    // Individuals
    //
    ///////////////////////////////////////////////////////////////////////////////////////
    -->


</rdf:RDF>