<?xml version="1.0"?>
<rdf:RDF
    xmlns:skos="http://www.w3.org/2004/02/skos/core#"
    xmlns:fibo-fnd-org-fm="http://www.omg.org/spec/EDMC-FIBO/FND/Organizations/FormalOrganizations/"
    xmlns:fibo-fnd-plc-loc="http://www.omg.org/spec/EDMC-FIBO/FND/Places/Locations/"
    xmlns:fibo-fnd-plc-cty="http://www.omg.org/spec/EDMC-FIBO/FND/Places/Countries/"
    xmlns:fibo-fnd-rel-rel="http://www.omg.org/spec/EDMC-FIBO/FND/Relations/Relations/"
    xmlns:fibo-fnd-law-cor="http://www.omg.org/spec/EDMC-FIBO/FND/Law/LegalCore/"
    xmlns:fibo-fnd-plc-adr="http://www.omg.org/spec/EDMC-FIBO/FND/Places/Addresses/"
    xmlns:fibo-fnd-gao-gl="http://www.omg.org/spec/EDMC-FIBO/FND/GoalsAndObjectives/Goals/"
    xmlns:sm="http://www.omg.org/techprocess/ab/SpecificationMetadata/"
    xmlns:fibo-fnd-utl-av="http://www.omg.org/spec/EDMC-FIBO/FND/Utilities/AnnotationVocabulary/"
    xmlns:rdf="http://www.w3.org/1999/02/22-rdf-syntax-ns#"
    xmlns:fibo-fnd-utl-bt="http://www.omg.org/spec/EDMC-FIBO/FND/Utilities/BusinessFacingTypes/"
    xmlns:owl="http://www.w3.org/2002/07/owl#"
    xmlns:dct="http://purl.org/dc/terms/"
    xmlns:fibo-fnd-org-org="http://www.omg.org/spec/EDMC-FIBO/FND/Organizations/Organizations/"
    xmlns:fibo-fnd-aap-agt="http://www.omg.org/spec/EDMC-FIBO/FND/AgentsAndPeople/Agents/"
    xmlns:xsd="http://www.w3.org/2001/XMLSchema#"
    xmlns:rdfs="http://www.w3.org/2000/01/rdf-schema#"
  xml:base="http://www.omg.org/spec/EDMC-FIBO/FND/Law/LegalCore/">
  <owl:Ontology rdf:about="">
    <sm:dependsOn rdf:datatype="http://www.w3.org/2001/XMLSchema#anyURI"
    >http://www.omg.org/spec/EDMC-FIBO/FND/GoalsAndObjectives/Goals/</sm:dependsOn>
    <sm:dependsOn rdf:datatype="http://www.w3.org/2001/XMLSchema#anyURI"
    >http://www.omg.org/techprocess/ab/SpecificationMetadata/</sm:dependsOn>
    <sm:dependsOn rdf:datatype="http://www.w3.org/2001/XMLSchema#anyURI"
    >http://www.omg.org/spec/EDMC-FIBO/FND/Utilities/AnnotationVocabulary/</sm:dependsOn>
    <owl:imports rdf:resource="http://www.omg.org/spec/EDMC-FIBO/FND/Organizations/FormalOrganizations/"/>
    <sm:keyword rdf:datatype="http://www.w3.org/2001/XMLSchema#string"
    >vocabulary</sm:keyword>
    <sm:moduleName rdf:datatype="http://www.w3.org/2001/XMLSchema#string"
    >Law</sm:moduleName>
    <sm:filename rdf:datatype="http://www.w3.org/2001/XMLSchema#string"
    >Legal Core Ontology</sm:filename>
    <sm:topicArea rdf:datatype="http://www.w3.org/2001/XMLSchema#string"
    >finance</sm:topicArea>
    <sm:fileAbbreviation rdf:datatype="http://www.w3.org/2001/XMLSchema#string"
    >fibo-fnd-law-cor</sm:fileAbbreviation>
    <sm:technologyArea rdf:datatype="http://www.w3.org/2001/XMLSchema#string"
    >formal semantics</sm:technologyArea>
    <sm:dependsOn rdf:datatype="http://www.w3.org/2001/XMLSchema#anyURI"
    >http://www.omg.org/spec/EDMC-FIBO/FND/Places/Locations/</sm:dependsOn>
    <sm:responsibleTaskForce rdf:datatype="http://www.w3.org/2001/XMLSchema#anyURI"
    >http://fdtf.omg.org/</sm:responsibleTaskForce>
    <sm:specificationURL rdf:datatype="http://www.w3.org/2001/XMLSchema#anyURI"
    >http://www.omg.org/spec/EDMC-FIBO/FND/</sm:specificationURL>
    <sm:contributor rdf:datatype="http://www.w3.org/2001/XMLSchema#string"
    >Adaptive, Inc.</sm:contributor>
    <sm:contentLanguage rdf:datatype="http://www.w3.org/2001/XMLSchema#anyURI"
    >http://www.omg.org/spec/ODM/</sm:contentLanguage>
    <sm:specificationAbbreviation rdf:datatype="http://www.w3.org/2001/XMLSchema#string"
    >FIBO-FND</sm:specificationAbbreviation>
    <sm:priorVersion rdf:datatype="http://www.w3.org/2001/XMLSchema#anyURI"
    >http://www.omg.org/spec/FIBO/Foundations/20130601/Law/LegalCore.owl</sm:priorVersion>
    <rdfs:label>Financial Industry Business Ontology (FIBO) Legal Core Ontology</rdfs:label>
    <sm:copyright rdf:datatype="http://www.w3.org/2001/XMLSchema#string"
    >Copyright (c) 2013 EDM Council, Inc.
Copyright (c) 2013 Object Management Group, Inc.</sm:copyright>
    <sm:publicationDate rdf:datatype="http://www.w3.org/2001/XMLSchema#dateTime"
    >2013-08-26T18:00:00</sm:publicationDate>
    <sm:familyAbstract rdf:datatype="http://www.w3.org/2001/XMLSchema#string"
    >The content that comprises the Financial Industry Business Ontology (FIBO) is documentation, interpretable in formal logic, of the concepts represented by finance industry terms as used in official financial organization documents such as contracts, product/service specifications and governance and regulatory compliance documents.</sm:familyAbstract>
    <sm:fileAbstract rdf:datatype="http://www.w3.org/2001/XMLSchema#string"
    >This ontology defines high-level legal concepts for use in other FIBO ontology elements. These concepts include law and constitution, both of which are framed at a more abstract level than national or state laws and constitutions, so that law forms the basis both for statutes and for company by-laws, and constitution forms the basis both for national or state constitutions and for instruments which are constitutive of incorporated legal entities. This ontology also defines some of the variants of these such as governmental constitutions and ordinances. Other types of law are provided in the Jurisdictions ontology as extensions of concepts in this ontology. Court of Law is also defined here.</sm:fileAbstract>
    <sm:thisVersion rdf:datatype="http://www.w3.org/2001/XMLSchema#string"
    >1.0 </sm:thisVersion>
    <dct:license rdf:datatype="http://www.w3.org/2001/XMLSchema#string"
    >The MIT License:  Permission is hereby granted, free of charge, to any person obtaining a copy of this software and associated documentation files (the "Software"), to deal in the Software without restriction, including without limitation the rights to use, copy, modify, merge, publish, distribute, sublicense, and/or sell copies of the Software, and to permit persons to whom the Software is furnished to do so, subject to the following conditions:

The copyright notice and this permission notice shall be included in all copies or substantial portions of the Software.

THE SOFTWARE IS PROVIDED "AS IS", WITHOUT WARRANTY OF ANY KIND, EXPRESS OR IMPLIED, INCLUDING BUT NOT LIMITED TO THE WARRANTIES OF MERCHANTABILITY, FITNESS FOR A PARTICULAR PURPOSE
AND NONINFRINGEMENT.  IN NO EVENT SHALL THE AUTHORS OR COPYRIGHT HOLDERS BE LIABLE FOR ANY CLAIM, DAMAGES OR OTHER LIABILITY, WHETHER IN AN ACTION OF CONTRACT, TORT OR OTHERWISE, ARISING FROM, OUT OF OR IN CONNECTION WITH THE SOFTWARE OR THE USE OR OTHER DEALINGS IN THE SOFTWARE.</dct:license>
    <sm:familyURL rdf:datatype="http://www.w3.org/2001/XMLSchema#anyURI"
    >http://www.omg.org/spec/EDMC-FIBO/</sm:familyURL>
    <sm:keyword rdf:datatype="http://www.w3.org/2001/XMLSchema#string"
    >FIBO</sm:keyword>
    <sm:dependsOn rdf:datatype="http://www.w3.org/2001/XMLSchema#anyURI"
    >http://www.omg.org/spec/EDMC-FIBO/FND/Organizations/FormalOrganizations/</sm:dependsOn>
    <sm:submitter rdf:datatype="http://www.w3.org/2001/XMLSchema#string"
    >EDM Council, Inc.</sm:submitter>
    <sm:keyword rdf:datatype="http://www.w3.org/2001/XMLSchema#string"
    >Financial Industry Business Ontology</sm:keyword>
    <sm:contributor rdf:datatype="http://www.w3.org/2001/XMLSchema#string"
    >Thematix Partners LLC</sm:contributor>
    <sm:dependsOn rdf:datatype="http://www.w3.org/2001/XMLSchema#anyURI"
    >http://www.omg.org/spec/EDMC-FIBO/FND/Places/Addresses/</sm:dependsOn>
    <sm:specificationVersionURL rdf:datatype="http://www.w3.org/2001/XMLSchema#anyURI"
    >http://www.omg.org/spec/EDMC-FIBO/FND/1.0/</sm:specificationVersionURL>
    <sm:addressForComments rdf:datatype="http://www.w3.org/2001/XMLSchema#anyURI"
    >http://www.omg.org/issues/</sm:addressForComments>
    <sm:dependsOn rdf:datatype="http://www.w3.org/2001/XMLSchema#anyURI"
    >http://www.omg.org/spec/EDMC-FIBO/FND/Organizations/Organizations/</sm:dependsOn>
    <sm:contentLanguage rdf:datatype="http://www.w3.org/2001/XMLSchema#anyURI"
    >http://www.w3.org/standards/techs/owl#w3c_all</sm:contentLanguage>
    <skos:changeNote rdf:datatype="http://www.w3.org/2001/XMLSchema#string"
    >This version of the ontology was revised in advance of the September 2013 New Brunswick, NJ meeting, as follows:
   (1) to use slash style URI/IRIss (also called 303 URIs, vs. hash style) as required to support server side processing 
   (2) to use version-independent IRIs for all definitions internally as opposed to version-specific IRIs
   (3) to change the file suffix from .owl to .rdf to increase usability in RDF tools
   (4) to use 4-level abbreviations and corresponding namespace prefixes for all FIBO ontologies, reflecting a family/specification/module/ontology structure
   (5) to incorporate changes to the specification metadata to support documentation at the family, specification, module, and ontology level, similar to the abbreviations.
   (6) to revise some of the text definitions using more formal sources.</skos:changeNote>
    <sm:specificationVersionStatus rdf:datatype="http://www.w3.org/2001/XMLSchema#string"
    >Request For Comments (RFC)</sm:specificationVersionStatus>
    <dct:license rdf:datatype="http://www.w3.org/2001/XMLSchema#anyURI"
    >http://opensource.org/licenses/mit-license.php</dct:license>
    <sm:moduleVersion rdf:datatype="http://www.w3.org/2001/XMLSchema#string"
    >1.0</sm:moduleVersion>
    <sm:familyTitle rdf:datatype="http://www.w3.org/2001/XMLSchema#string"
    >Financial Industry Business Ontology (FIBO)</sm:familyTitle>
    <sm:moduleAbbreviation rdf:datatype="http://www.w3.org/2001/XMLSchema#string"
    >FIBO-FND-LAW</sm:moduleAbbreviation>
    <sm:dependsOn rdf:datatype="http://www.w3.org/2001/XMLSchema#anyURI"
    >http://www.omg.org/spec/EDMC-FIBO/FND/Utilities/BusinessFacingTypes/</sm:dependsOn>
    <sm:dependsOn rdf:datatype="http://www.w3.org/2001/XMLSchema#anyURI"
    >http://www.omg.org/spec/EDMC-FIBO/FND/AgentsAndPeople/Agents/</sm:dependsOn>
    <sm:keyword rdf:datatype="http://www.w3.org/2001/XMLSchema#string"
    >ontology</sm:keyword>
    <sm:specificationAbstract rdf:datatype="http://www.w3.org/2001/XMLSchema#string"
    >FIBO Foundations is a set of business concepts which are intended to support the financial industry terms semantics presented in other FIBO specifications.  

The FIBO Foundations models define concepts which are not unique to the financial services industry. From these, financial industry terms in other FIBO specifications may be derived by extension. Terms are also included which may be referred to by properties of things in those specifications. FIBO Foundations therefore includes a number of basic terms about legal, contractual and organizational concepts, among others. </sm:specificationAbstract>
    <skos:historyNote rdf:datatype="http://www.w3.org/2001/XMLSchema#string"
    >This version of the FIBO Foundations Specification was revised primarily to reflect comments received at the March 2013 OMG Technical Meeting in Reston and reflected in the Errata discussed at the June 2013 OMG Technical Meeting in Berlin. 

Revisions to FIBO Foundations are managed per the process outlined in the Policies and Procedures for OMG standards, with the intent to maintain backwards compatibility in the ontologies to the degree possible.
  
The RDF/XML serialized OWL for the Foundations ODM/OWL ontologies have been checked for syntactic errors and logical consistency with Protege 4 (http://protege.stanford.edu/), HermiT 1.3.7 (http://www.hermit-reasoner.com/) and Pellet 2.2 (http://clarkparsia.com/pellet/).</skos:historyNote>
    <owl:versionIRI rdf:datatype="http://www.w3.org/2001/XMLSchema#anyURI"
    >http://www.omg.org/spec/EDMC-FIBO/FND/20130801/Law/LegalCore/</owl:versionIRI>
    <sm:dependsOn rdf:datatype="http://www.w3.org/2001/XMLSchema#anyURI"
    >http://www.omg.org/spec/EDMC-FIBO/FND/Places/Countries/</sm:dependsOn>
    <sm:familyAbbreviation rdf:datatype="http://www.w3.org/2001/XMLSchema#string"
    >FIBO</sm:familyAbbreviation>
    <sm:specificationTitle rdf:datatype="http://www.w3.org/2001/XMLSchema#string"
    >Financial Industry Business Ontology (FIBO) Foundations Specification</sm:specificationTitle>
    <sm:moduleAbstract rdf:datatype="http://www.w3.org/2001/XMLSchema#string"
    >This module includes several ontologies defining legal concepts, including constitutions, laws and jurisdictions. It also includes the definition of legal capacities such as signatory capacity, contractual capability and the like.</sm:moduleAbstract>
    <sm:keyword rdf:datatype="http://www.w3.org/2001/XMLSchema#string"
    >foundational vocabulary</sm:keyword>
    <sm:dependsOn rdf:datatype="http://www.w3.org/2001/XMLSchema#anyURI"
    >http://www.omg.org/spec/EDMC-FIBO/FND/Relations/Relations/</sm:dependsOn>
  </owl:Ontology>
  <owl:Class rdf:about="http://www.omg.org/spec/EDMC-FIBO/FND/Law/LegalCore/Law">
    <skos:editorialNote>Any law or body of law, which may have force in some context, including national laws, company bylaws and the like.</skos:editorialNote>
    <fibo-fnd-utl-av:definitionOrigin>http://en.wikipedia.org/wiki/Law</fibo-fnd-utl-av:definitionOrigin>
    <skos:definition>Law is a term which does not have a universally accepted definition, but one definition is that law is a system of rules and guidelines which are enforced through social institutions to govern behavior. Laws are made by governments, specifically by their legislatures.  The formation of laws themselves may be influenced by a constitution (written or unwritten) and the rights encoded therein.  The law shapes politics, economics and society in countless ways and serves as a social mediator of relations between people.</skos:definition>
    <rdfs:label>Law</rdfs:label>
  </owl:Class>
  <owl:Class rdf:about="http://www.omg.org/spec/EDMC-FIBO/FND/Law/LegalCore/CourtOfLaw">
    <rdfs:subClassOf rdf:resource="http://www.omg.org/spec/EDMC-FIBO/FND/Organizations/FormalOrganizations/FormalOrganization"/>
    <fibo-fnd-utl-av:definitionOrigin>Merriam-Webster Online Dictionary</fibo-fnd-utl-av:definitionOrigin>
    <skos:definition>A court of law is a court that hears cases and decides them on the basis of statutes or the common law.</skos:definition>
    <rdfs:label>court of law</rdfs:label>
  </owl:Class>
  <owl:Class rdf:about="http://www.omg.org/spec/EDMC-FIBO/FND/Law/LegalCore/Ordinance">
    <rdfs:subClassOf rdf:resource="http://www.omg.org/spec/EDMC-FIBO/FND/Law/LegalCore/Law"/>
    <skos:definition>An authoritative rule or law; a decree or command; a public injunction or regulation, such as a city ordinance against excessive horn blowing. (Source: Dictionary.com)</skos:definition>
    <rdfs:label>ordinance</rdfs:label>
  </owl:Class>
  <owl:Class rdf:about="http://www.omg.org/spec/EDMC-FIBO/FND/Law/LegalCore/Constitution">
    <rdfs:subClassOf>
      <owl:Restriction>
        <owl:allValuesFrom rdf:resource="http://www.omg.org/spec/EDMC-FIBO/FND/Law/LegalCore/Law"/>
        <owl:onProperty rdf:resource="http://www.omg.org/spec/EDMC-FIBO/FND/Relations/Relations/governs"/>
      </owl:Restriction>
    </rdfs:subClassOf>
    <fibo-fnd-utl-av:definitionOrigin>Merriam-Webster Online Dictionary</fibo-fnd-utl-av:definitionOrigin>
    <skos:editorialNote>This defines the framework in which laws (for a country constitution), rules and regulations (for a party or organization constitution) or contractual commitments are made and in which they have force.</skos:editorialNote>
    <skos:definition>A constitution defines the basic principles and laws of a nation, state, or social group that determine the powers and duties of the government and guarantee certain rights to the people in it.</skos:definition>
    <rdfs:label>constitution</rdfs:label>
  </owl:Class>
  <owl:Class rdf:about="http://www.omg.org/spec/EDMC-FIBO/FND/Law/LegalCore/GovernmentalConstitution">
    <rdfs:subClassOf rdf:resource="http://www.omg.org/spec/EDMC-FIBO/FND/Law/LegalCore/Constitution"/>
    <skos:editorialNote>This defines the framework in which laws are made and in which they have force.</skos:editorialNote>
    <fibo-fnd-utl-av:definitionOrigin>http://en.wikipedia.org/wiki/Constitution#Governmental_constitutions</fibo-fnd-utl-av:definitionOrigin>
    <skos:definition>Most commonly, the term constitution refers to a set of rules and principles that define the nature and extent of government.  Most constitutions seek to regulate the relationship between institutions of the state, in a basic sense the relationship between the executive, legislature and the judiciary, but also the relationship of institutions within those branches.  For example, executive branches can be divided into a head of government, government departments/ministries, executive agencies and a civil service/administration.  Most constitutions also attempt to define the relationship between individuals and the state, and to establish the broad rights of individual citizens. It is thus the most basic law of a territory from which all the other laws and rules are hierarchically derived; in some territories it is in fact called Basic Law.</skos:definition>
    <rdfs:label>governmental constitution</rdfs:label>
  </owl:Class>
</rdf:RDF>

<!-- Created with TopBraid -->
