<?xml version="1.0" encoding="UTF-8"?>
<rdf:RDF xmlns:xsd="http://www.w3.org/2001/XMLSchema#"
         xmlns:sm="http://www.omg.org/techprocess/ab/SpecificationMetadata/"
         xmlns:fibo-fnd-utl-av="http://www.omg.org/spec/EDMC-FIBO/FND/Utilities/AnnotationVocabulary/"
         xmlns:rdf="http://www.w3.org/1999/02/22-rdf-syntax-ns#"
         xmlns:rdfs="http://www.w3.org/2000/01/rdf-schema#"
         xmlns:owl="http://www.w3.org/2002/07/owl#"
         xmlns:skos="http://www.w3.org/2004/02/skos/core#"
         xmlns:dc="http://purl.org/dc/terms/"
         xml:base="http://www.edmcouncil.org/spec/EDMC-SR/FND/Relative/RelativeBusinessEntities/">

   <owl:Ontology rdf:about="http://www.edmcouncil.org/spec/EDMC-SR/FND/Relative/RelativeBusinessEntities/">
      <owl:imports rdf:resource="http://www.edmcouncil.org/spec/EDMC-SR/UO/OntologicalDegree/"/>
   </owl:Ontology>

   <!--Datatypes-->

<!--Object Properties-->

<owl:ObjectProperty rdf:about="http://www.edmcouncil.org/spec/EDMC-SR/FND/Relative/RelativeBusinessEntities/relativeBusinessEntityDefinedInContextOf">
      <skos:definition>The context in which the Relative Business Entity is defined and in which some entity performs the defined role.</skos:definition>
      <rdfs:subPropertyOf rdf:resource="http://www.edmcouncil.org/spec/EDMC-SR/UO/OntologicalDegree/inContext"/>
      <rdfs:domain rdf:resource="http://www.edmcouncil.org/spec/EDMC-SR/FND/Relative/RelativeBusinessEntities/RelativeBusinessEntity"/>
      <rdfs:range rdf:resource="http://www.edmcouncil.org/spec/EDMC-SR/FND/Relative/RelativeBusinessEntities/BusinessContext"/>
   </owl:ObjectProperty>

   <owl:ObjectProperty rdf:about="http://www.edmcouncil.org/spec/EDMC-SR/FND/Relative/RelativeBusinessEntities/takesEntityForm">
      <skos:definition>The form which a Relative Business Entity takes. This may be an Autonomous Agent.</skos:definition>
      <rdfs:subPropertyOf rdf:resource="http://www.omg.org/spec/EDMC-SR/FND/OwnershipAndControl/Ownership/takesForm"/>
      <rdfs:domain rdf:resource="http://www.edmcouncil.org/spec/EDMC-SR/FND/Relative/RelativeBusinessEntities/RelativeBusinessEntity"/>
      <rdfs:range rdf:resource="http://www.omg.org/spec/EDMC-SR/FND/AgentsAndPeople/Agents/AutonomousAgent"/>
   </owl:ObjectProperty>

   <!--Data Properties-->

<!--Annotation Properties-->

<!--Classes-->

<owl:Class rdf:about="http://www.edmcouncil.org/spec/EDMC-SR/FND/Relative/RelativeBusinessEntities/BusinessContext">
      <rdfs:label>Business Context</rdfs:label>
      <rdfs:subClassOf rdf:resource="http://www.edmcouncil.org/spec/EDMC-SR/UO/OntologicalDegree/MediatingThing"/>
   </owl:Class>

   <owl:Class rdf:about="http://www.edmcouncil.org/spec/EDMC-SR/FND/Relative/RelativeBusinessEntities/RelativeBusinessEntity">
      <rdfs:label>Relative Business Entity</rdfs:label>
      <skos:definition>A business entity defined in some relative sense, for example by reference to its role in some process or its overall role or function in the marketplace or in the world as a whole.</skos:definition>
      <rdfs:subClassOf rdf:resource="http://www.edmcouncil.org/spec/EDMC-SR/UO/OntologicalDegree/RelativeThing"/>
   </owl:Class>

   <!--Individuals-->

</rdf:RDF>