<?xml version="1.0" encoding="UTF-8"?>
<!DOCTYPE rdf:RDF [
	<!ENTITY dct "http://purl.org/dc/terms/">
	<!ENTITY fibo-fnd-plc-adr "https://spec.edmcouncil.org/fibo/FND/Places/Addresses/">
	<!ENTITY fibo-fnd-plc-fac "https://spec.edmcouncil.org/fibo/FND/Places/Facilities/">
	<!ENTITY fibo-fnd-plc-loc "https://spec.edmcouncil.org/fibo/FND/Places/Locations/">
	<!ENTITY fibo-fnd-pty-rl "https://spec.edmcouncil.org/fibo/FND/Parties/Roles/">
	<!ENTITY fibo-fnd-rel-rel "https://spec.edmcouncil.org/fibo/FND/Relations/Relations/">
	<!ENTITY fibo-fnd-utl-av "https://spec.edmcouncil.org/fibo/FND/Utilities/AnnotationVocabulary/">
	<!ENTITY owl "http://www.w3.org/2002/07/owl#">
	<!ENTITY rdf "http://www.w3.org/1999/02/22-rdf-syntax-ns#">
	<!ENTITY rdfs "http://www.w3.org/2000/01/rdf-schema#">
	<!ENTITY skos "http://www.w3.org/2004/02/skos/core#">
	<!ENTITY sm "http://www.omg.org/techprocess/ab/SpecificationMetadata/">
	<!ENTITY xsd "http://www.w3.org/2001/XMLSchema#">
]>
<rdf:RDF
	xml:base="https://spec.edmcouncil.org/fibo/FND/Places/Facilities/"
	xmlns:dct="http://purl.org/dc/terms/"
	xmlns:fibo-fnd-plc-adr="https://spec.edmcouncil.org/fibo/FND/Places/Addresses/"
	xmlns:fibo-fnd-plc-fac="https://spec.edmcouncil.org/fibo/FND/Places/Facilities/"
	xmlns:fibo-fnd-plc-loc="https://spec.edmcouncil.org/fibo/FND/Places/Locations/"
	xmlns:fibo-fnd-pty-rl="https://spec.edmcouncil.org/fibo/FND/Parties/Roles/"
	xmlns:fibo-fnd-rel-rel="https://spec.edmcouncil.org/fibo/FND/Relations/Relations/"
	xmlns:fibo-fnd-utl-av="https://spec.edmcouncil.org/fibo/FND/Utilities/AnnotationVocabulary/"
	xmlns:owl="http://www.w3.org/2002/07/owl#"
	xmlns:rdf="http://www.w3.org/1999/02/22-rdf-syntax-ns#"
	xmlns:rdfs="http://www.w3.org/2000/01/rdf-schema#"
	xmlns:skos="http://www.w3.org/2004/02/skos/core#"
	xmlns:sm="http://www.omg.org/techprocess/ab/SpecificationMetadata/"
	xmlns:xsd="http://www.w3.org/2001/XMLSchema#">
	
	<owl:Ontology
		rdf:about="https://spec.edmcouncil.org/fibo/FND/Places/Facilities/">
		<rdfs:label>Facilities Ontology</rdfs:label>
		<dct:license
			rdf:datatype="&xsd;anyURI">http://www.omg.org/techprocess/ab/SpecificationMetadata/MITLicense</dct:license>
		<sm:contentLanguage
			rdf:datatype="&xsd;anyURI">http://www.omg.org/spec/ODM/</sm:contentLanguage>
		<sm:contentLanguage
			rdf:datatype="&xsd;anyURI">http://www.w3.org/standards/techs/owl#w3c_all</sm:contentLanguage>
		<sm:copyright>Copyright (c) 2014 EDM Council, Inc.
Copyright (c) 2014 Object Management Group, Inc.</sm:copyright>
		<sm:dependsOn
			rdf:datatype="&xsd;anyURI">https://spec.edmcouncil.org/fibo/FND/Parties/Roles/</sm:dependsOn>
		<sm:dependsOn
			rdf:datatype="&xsd;anyURI">https://spec.edmcouncil.org/fibo/FND/Places/Addresses/</sm:dependsOn>
		<sm:dependsOn
			rdf:datatype="&xsd;anyURI">https://spec.edmcouncil.org/fibo/FND/Places/Locations/</sm:dependsOn>
		<sm:dependsOn
			rdf:datatype="&xsd;anyURI">https://spec.edmcouncil.org/fibo/FND/Relations/Relations/</sm:dependsOn>
		<sm:dependsOn
			rdf:datatype="&xsd;anyURI">https://spec.edmcouncil.org/fibo/FND/Utilities/AnnotationVocabulary/</sm:dependsOn>
		<sm:fileAbbreviation>fibo-fnd-plc-fac</sm:fileAbbreviation>
		<sm:fileAbstract>This ontology provides scaffolding for use in describing concepts related to facilities, both virtual and physical, including physical sites that provide various facilities.</sm:fileAbstract>
		<sm:filename>Facilities.rdf</sm:filename>
		<rdfs:seeAlso
			rdf:datatype="&xsd;anyURI">https://spec.edmcouncil.org/fibo/AboutTheEDMC-FIBOFamily/</rdfs:seeAlso>
		<rdfs:seeAlso
			rdf:datatype="&xsd;anyURI">https://spec.edmcouncil.org/fibo/FND/AboutFND/</rdfs:seeAlso>
		<rdfs:seeAlso
			rdf:datatype="&xsd;anyURI">https://spec.edmcouncil.org/fibo/FND/Places/AboutPlaces/</rdfs:seeAlso>
		<owl:imports
			rdf:resource="https://spec.edmcouncil.org/fibo/FND/Parties/Roles/"/>
		<owl:imports
			rdf:resource="https://spec.edmcouncil.org/fibo/FND/Places/Addresses/"/>
		<owl:imports
			rdf:resource="https://spec.edmcouncil.org/fibo/FND/Places/Locations/"/>
		<owl:imports
			rdf:resource="https://spec.edmcouncil.org/fibo/FND/Relations/Relations/"/>
		<owl:imports
			rdf:resource="https://spec.edmcouncil.org/fibo/FND/Utilities/AnnotationVocabulary/"/>
		<owl:versionIRI
			rdf:resource="https://spec.edmcouncil.org/fibo/FND/20141101/Places/Facilities/"/>
		<skos:changeNote>This ontology was added to Foundations in advance of the December 2014 Long Beach meeting in support of the SEC specification.</skos:changeNote>
	</owl:Ontology>
	
	<owl:Class
		rdf:about="&fibo-fnd-plc-fac;Capability">
		<rdfs:subClassOf>
			<owl:Restriction>
				<owl:onProperty
					rdf:resource="&fibo-fnd-rel-rel;involves"/>
				<owl:someValuesFrom
					rdf:resource="&fibo-fnd-plc-fac;Facility"/>
			</owl:Restriction>
		</rdfs:subClassOf>
		<rdfs:label>capability</rdfs:label>
		<skos:definition>A capability represents the ability to perform a particular type of work and may involve people with particular skills and knowledge, intellectual property, defined practices, operating facilities, tools and equipment.</skos:definition>
		<fibo-fnd-utl-av:adaptedFrom>Value Delivery Modeling Language Specification, http://www.omg.org/spec/VDML/</fibo-fnd-utl-av:adaptedFrom>
	</owl:Class>
	
	<owl:Class
		rdf:about="&fibo-fnd-plc-fac;Facility">
		<rdfs:subClassOf
			rdf:resource="&fibo-fnd-pty-rl;ThingInRole"/>
		<rdfs:subClassOf>
			<owl:Restriction>
				<owl:allValuesFrom
					rdf:resource="&fibo-fnd-plc-fac;Site"/>
				<owl:onProperty
					rdf:resource="&fibo-fnd-plc-fac;isSituatedAt"/>
			</owl:Restriction>
		</rdfs:subClassOf>
		<rdfs:subClassOf>
			<owl:Restriction>
				<owl:onProperty
					rdf:resource="&fibo-fnd-rel-rel;provides"/>
				<owl:someValuesFrom
					rdf:resource="&fibo-fnd-plc-fac;Capability"/>
			</owl:Restriction>
		</rdfs:subClassOf>
		<rdfs:label>facility</rdfs:label>
		<skos:definition>something that is built, contrived, established, or installed to serve a particular purpose, or make some course of action or operation easier, or provide some capability or service</skos:definition>
		<fibo-fnd-utl-av:explanatoryNote>A facility may be concrete (as in a manufacturing facility) or abstract. Concrete facilities may be permanent, semi-permanent, or temporary structures, providing one or more capabilities at a given site.  A single site may include multiple facilities and a given facility may span multiple sites.</fibo-fnd-utl-av:explanatoryNote>
	</owl:Class>
	
	<owl:Class
		rdf:about="&fibo-fnd-plc-fac;PhysicalSite">
		<rdfs:subClassOf
			rdf:resource="&fibo-fnd-plc-fac;Site"/>
		<rdfs:subClassOf>
			<owl:Restriction>
				<owl:onClass
					rdf:resource="&fibo-fnd-plc-adr;Address"/>
				<owl:onProperty
					rdf:resource="&fibo-fnd-rel-rel;hasIdentity"/>
				<owl:qualifiedCardinality
					rdf:datatype="&xsd;nonNegativeInteger">1</owl:qualifiedCardinality>
			</owl:Restriction>
		</rdfs:subClassOf>
		<rdfs:subClassOf>
			<owl:Restriction>
				<owl:onClass
					rdf:resource="&fibo-fnd-plc-loc;PhysicalLocation"/>
				<owl:onProperty
					rdf:resource="&fibo-fnd-plc-loc;isLocatedAt"/>
				<owl:qualifiedCardinality
					rdf:datatype="&xsd;nonNegativeInteger">1</owl:qualifiedCardinality>
			</owl:Restriction>
		</rdfs:subClassOf>
		<rdfs:label>physical site</rdfs:label>
		<skos:definition>A physical site is a an actual location that situates something, typically a structure or building, archeological dig, landing location for an aircraft or spacecraft, etc.  From biology, this could also be the site of a wound, and active site, and so forth. A physical site has certain characteristics that contribute to the context it provides, including area, shape, accessibility, and in the case of a geographic site, landforms, soil and ground conditions, climate, and so forth.</skos:definition>
	</owl:Class>
	
	<owl:Class
		rdf:about="&fibo-fnd-plc-fac;Site">
		<rdfs:subClassOf
			rdf:resource="&fibo-fnd-pty-rl;ThingInRole"/>
		<rdfs:subClassOf>
			<owl:Restriction>
				<owl:onClass
					rdf:resource="&fibo-fnd-plc-loc;Location"/>
				<owl:onProperty
					rdf:resource="&fibo-fnd-plc-loc;isLocatedAt"/>
				<owl:qualifiedCardinality
					rdf:datatype="&xsd;nonNegativeInteger">1</owl:qualifiedCardinality>
			</owl:Restriction>
		</rdfs:subClassOf>
		<rdfs:subClassOf>
			<owl:Restriction>
				<owl:onProperty
					rdf:resource="&fibo-fnd-pty-rl;isPlayedBy"/>
				<owl:someValuesFrom>
					<owl:Restriction>
						<owl:allValuesFrom
							rdf:resource="&owl;Thing"/>
						<owl:onProperty
							rdf:resource="&fibo-fnd-plc-fac;situates"/>
					</owl:Restriction>
				</owl:someValuesFrom>
			</owl:Restriction>
		</rdfs:subClassOf>
		<rdfs:label>site</rdfs:label>
		<skos:definition>A site is a place, setting, or context in which something is situated.</skos:definition>
	</owl:Class>
	
	<owl:Class
		rdf:about="&fibo-fnd-plc-fac;Venue">
		<rdfs:subClassOf
			rdf:resource="&fibo-fnd-plc-fac;Site"/>
		<rdfs:subClassOf>
			<owl:Restriction>
				<owl:minCardinality
					rdf:datatype="&xsd;nonNegativeInteger">1</owl:minCardinality>
				<owl:onProperty
					rdf:resource="&fibo-fnd-rel-rel;hasContext"/>
			</owl:Restriction>
		</rdfs:subClassOf>
		<rdfs:label>venue</rdfs:label>
		<skos:definition>A place where something happens, described in the context of the event or activity that occurs there</skos:definition>
	</owl:Class>
	
	<rdf:Description
		rdf:about="&fibo-fnd-plc-fac;hasLatitude">
		<rdf:type
			rdf:resource="&owl;DatatypeProperty"/>
		<rdf:type
			rdf:resource="&owl;FunctionalProperty"/>
		<rdfs:label>has latitude</rdfs:label>
		<sm:directSource>The National Atlas, nationalatlas.gov/articles/mapping/a_latlong.html</sm:directSource>
		<rdfs:range
			rdf:resource="&xsd;string"/>
		<skos:definition>Latitude values indicate the angular distance between the Equator and points north or south of it on the surface of the Earth.</skos:definition>
	</rdf:Description>
	
	<rdf:Description
		rdf:about="&fibo-fnd-plc-fac;hasLongitude">
		<rdf:type
			rdf:resource="&owl;DatatypeProperty"/>
		<rdf:type
			rdf:resource="&owl;FunctionalProperty"/>
		<rdfs:label>has longitude</rdfs:label>
		<sm:directSource>The National Atlas, nationalatlas.gov/articles/mapping/a_latlong.html</sm:directSource>
		<rdfs:range
			rdf:resource="&xsd;string"/>
		<skos:definition>Lines of longitude, called meridians, run perpendicular to lines of latitude, and all pass through both poles. Longitude values indicate the angular distance between the Prime Meridian and points east or west of it on the surface of the Earth.</skos:definition>
	</rdf:Description>
	
	<owl:ObjectProperty
		rdf:about="&fibo-fnd-plc-fac;isSituatedAt">
		<rdfs:label>is situated at</rdfs:label>
		<skos:definition>indicates that something has been positioned, located or placed at some site, or in some setting, situation, or context</skos:definition>
	</owl:ObjectProperty>
	
	<owl:ObjectProperty
		rdf:about="&fibo-fnd-plc-fac;situates">
		<rdfs:label>situates</rdfs:label>
		<owl:inverseOf
			rdf:resource="&fibo-fnd-plc-fac;isSituatedAt"/>
		<skos:definition>indicates the place, setting, or context in which something is situated</skos:definition>
	</owl:ObjectProperty>

</rdf:RDF>