<?xml version="1.0" encoding="UTF-8"?>
  
<!DOCTYPE rdf:RDF [
    <!ENTITY fibo-sec-dbt-dbt-ins "http://spec.edmcouncil.org/fibo/red/sec/debt/debt-foundations/debt-instruments/">
    <!ENTITY fibo-fnd-acc-dbt "http://spec.edmcouncil.org/fibo/red/fnd/accounting/debt-terms/">
    <!ENTITY fibo-fnd-agr-ctr "http://spec.edmcouncil.org/fibo/red/fnd/agreements/contracts/">
    <!ENTITY fibo-sec-sec-sec "http://spec.edmcouncil.org/fibo/red/sec/securities/securities/">
    <!ENTITY fibo-sec-dbt-mm-repo "http://spec.edmcouncil.org/fibo/red/sec/debt/money-markets/repo/">
    <!ENTITY fibo-sec-dbt-mm-tr "http://spec.edmcouncil.org/fibo/red/sec/debt/money-markets/traded-short-term-debt/">
    <!ENTITY fibo-loan-loan-bt "http://spec.edmcouncil.org/fibo/red/loan/loans/loan-basic-terms/">
    <!ENTITY fibo-fnd-utl-bt "http://spec.edmcouncil.org/fibo/red/fnd/utilities/business-facing-types/">
    <!ENTITY fibo-fnd-acc-cur "http://spec.edmcouncil.org/fibo/red/fnd/accounting/currency-amount/">
    <!ENTITY fibo-sec-dbt-dbt-cfl "http://spec.edmcouncil.org/fibo/red/sec/debt/debt-foundations/debt-cashflow-terms/">
    <!ENTITY fibo-sec-dbt-dbt-par "http://spec.edmcouncil.org/fibo/red/sec/debt/debt-foundations/parity-variants/">
    <!ENTITY fibo-fnd-tim-tim "http://spec.edmcouncil.org/fibo/red/fnd/date-time/date-time/">
]>

<rdf:RDF xmlns:xsd="http://www.w3.org/2001/XMLSchema#"
         xmlns:sm="http://www.omg.org/techprocess/ab/SpecificationMetadata/"
         xmlns:xs="http://www.w3.org/2001/XMLSchema"
         xmlns:fibo-fnd-utl-av="http://www.omg.org/spec/EDMC-FIBO/FND/Utilities/AnnotationVocabulary/"
         xmlns:rdf="http://www.w3.org/1999/02/22-rdf-syntax-ns#"
         xmlns:rdfs="http://www.w3.org/2000/01/rdf-schema#"
         xmlns:owl="http://www.w3.org/2002/07/owl#"
         xmlns:skos="http://www.w3.org/2004/02/skos/core#"
         xmlns:dc="http://purl.org/dc/terms/"
         xml:base="http://spec.edmcouncil.org/fibo/red/sec/debt/debt-foundations/debt-instruments/">

   <owl:Ontology rdf:about="http://spec.edmcouncil.org/fibo/red/sec/debt/debt-foundations/debt-instruments/">
      <owl:imports rdf:resource="http://spec.edmcouncil.org/fibo/red/fnd/accounting/debt-terms/"/>
      <owl:imports rdf:resource="http://spec.edmcouncil.org/fibo/red/fnd/agreements/contracts/"/>
      <owl:imports rdf:resource="http://spec.edmcouncil.org/fibo/red/sec/securities/securities/"/>
      <owl:imports rdf:resource="http://spec.edmcouncil.org/fibo/red/sec/debt/money-markets/repo/"/>
      <owl:imports rdf:resource="http://spec.edmcouncil.org/fibo/red/sec/debt/money-markets/traded-short-term-debt/"/>
      <owl:imports rdf:resource="http://spec.edmcouncil.org/fibo/red/loan/loans/loan-basic-terms/"/>
      <owl:imports rdf:resource="http://spec.edmcouncil.org/fibo/red/fnd/utilities/business-facing-types/"/>
      <owl:imports rdf:resource="http://spec.edmcouncil.org/fibo/red/fnd/accounting/currency-amount/"/>
      <owl:imports rdf:resource="http://spec.edmcouncil.org/fibo/red/sec/debt/debt-foundations/debt-cashflow-terms/"/>
      <owl:imports rdf:resource="http://spec.edmcouncil.org/fibo/red/sec/debt/debt-foundations/parity-variants/"/>
      <owl:imports rdf:resource="http://spec.edmcouncil.org/fibo/red/fnd/date-time/date-time/"/>
   </owl:Ontology>


  <!--
    ///////////////////////////////////////////////////////////////////////////////////////
    //
    // Datatypes
    //
    ///////////////////////////////////////////////////////////////////////////////////////
    -->


<rdfs:Datatype rdf:about="&fibo-sec-dbt-dbt-ins;DayCountBasis">
      <skos:definition>The Interest Accrual Basis which is used to calculate interest on a debt or Debt security.</skos:definition>
      <owl:equivalentClass>
         <rdfs:Datatype>
            <owl:oneOf>
               <rdf:Description>
                  <rdf:first rdf:datatype="http://www.w3.org/2001/XMLSchema#string">30/360</rdf:first>
                  <rdf:rest>
                     <rdf:Description>
                        <rdf:first rdf:datatype="http://www.w3.org/2001/XMLSchema#string">Actual IM</rdf:first>
                        <rdf:rest>
                           <rdf:Description>
                              <rdf:first rdf:datatype="http://www.w3.org/2001/XMLSchema#string">Actual/360</rdf:first>
                              <rdf:rest>
                                 <rdf:Description>
                                    <rdf:first rdf:datatype="http://www.w3.org/2001/XMLSchema#string">Actual/365</rdf:first>
                                    <rdf:rest>
                                       <rdf:Description>
                                          <rdf:first rdf:datatype="http://www.w3.org/2001/XMLSchema#string">Actual/365L</rdf:first>
                                          <rdf:rest>
                                             <rdf:Description>
                                                <rdf:first rdf:datatype="http://www.w3.org/2001/XMLSchema#string">IC 30/Actual</rdf:first>
                                                <rdf:rest>
                                                   <rdf:Description>
                                                      <rdf:first rdf:datatype="http://www.w3.org/2001/XMLSchema#string">Actual/Actual AFB</rdf:first>
                                                      <rdf:rest>
                                                         <rdf:Description>
                                                            <rdf:first rdf:datatype="http://www.w3.org/2001/XMLSchema#string">Eurobond</rdf:first>
                                                            <rdf:rest>
                                                               <rdf:Description>
                                                                  <rdf:first rdf:datatype="http://www.w3.org/2001/XMLSchema#string">IC 30/360</rdf:first>
                                                                  <rdf:rest>
                                                                     <rdf:Description>
                                                                        <rdf:first rdf:datatype="http://www.w3.org/2001/XMLSchema#string">IC 30/360 ICMA</rdf:first>
                                                                        <rdf:rest>
                                                                           <rdf:Description>
                                                                              <rdf:first rdf:datatype="http://www.w3.org/2001/XMLSchema#string">IC 30/365</rdf:first>
                                                                              <rdf:rest>
                                                                                 <rdf:Description>
                                                                                    <rdf:first rdf:datatype="http://www.w3.org/2001/XMLSchema#string">Actual/Actual</rdf:first>
                                                                                    <rdf:rest rdf:resource="http://www.w3.org/1999/02/22-rdf-syntax-ns#nil"/>
                                                                                 </rdf:Description>
                                                                              </rdf:rest>
                                                                           </rdf:Description>
                                                                        </rdf:rest>
                                                                     </rdf:Description>
                                                                  </rdf:rest>
                                                               </rdf:Description>
                                                            </rdf:rest>
                                                         </rdf:Description>
                                                      </rdf:rest>
                                                   </rdf:Description>
                                                </rdf:rest>
                                             </rdf:Description>
                                          </rdf:rest>
                                       </rdf:Description>
                                    </rdf:rest>
                                 </rdf:Description>
                              </rdf:rest>
                           </rdf:Description>
                        </rdf:rest>
                     </rdf:Description>
                  </rdf:rest>
               </rdf:Description>
            </owl:oneOf>
         </rdfs:Datatype>
      </owl:equivalentClass>
   </rdfs:Datatype>


  <!--
    ///////////////////////////////////////////////////////////////////////////////////////
    //
    // Object Properties
    //
    ///////////////////////////////////////////////////////////////////////////////////////
    -->


<owl:ObjectProperty rdf:about="&fibo-sec-dbt-dbt-ins;hasCallTerms">
      <rdfs:label>has call terms</rdfs:label>
      <rdfs:domain rdf:resource="&fibo-sec-dbt-dbt-ins;.UnionClass.7"/>
      <rdfs:range rdf:resource="&fibo-sec-dbt-dbt-cfl;DebtCallTermsSet"/>
   </owl:ObjectProperty>

   <owl:ObjectProperty rdf:about="&fibo-sec-dbt-dbt-ins;relatesTo">
      <rdfs:label>relates to</rdfs:label>
      <rdfs:domain rdf:resource="&fibo-sec-dbt-dbt-ins;.UnionClass.7"/>
      <rdfs:range rdf:resource="&fibo-sec-dbt-dbt-ins;IssuedDebt"/>
   </owl:ObjectProperty>

   <owl:ObjectProperty rdf:about="&fibo-sec-dbt-dbt-ins;debtAmount">
      <rdfs:label>debt amount</rdfs:label>
      <skos:definition>The monetary amount of the debt that is securitized.</skos:definition>
      <rdfs:domain rdf:resource="&fibo-sec-dbt-dbt-ins;IssuedDebt"/>
      <rdfs:range rdf:resource="&fibo-fnd-acc-cur;MoneyAmount"/>
   </owl:ObjectProperty>

   <owl:ObjectProperty rdf:about="&fibo-sec-dbt-dbt-ins;hasRedemptionTerms">
      <rdfs:label>has redemption terms</rdfs:label>
      <rdfs:subPropertyOf rdf:resource="&fibo-fnd-agr-ctr;contractHasTerms"/>
      <rdfs:domain rdf:resource="&fibo-sec-dbt-dbt-ins;NonTradableDebtInstrument"/>
      <rdfs:range rdf:resource="&fibo-sec-dbt-mm-tr;NonTradableDebtRedemptionTerms"/>
   </owl:ObjectProperty>

   <owl:ObjectProperty rdf:about="&fibo-sec-dbt-dbt-ins;definesTermsFor">
      <rdfs:label>defines terms for</rdfs:label>
      <rdfs:subPropertyOf rdf:resource="&fibo-sec-dbt-dbt-ins;relatesTo"/>
      <rdfs:subPropertyOf rdf:resource="&fibo-loan-loan-bt;setsOutTermsFor"/>
      <rdfs:domain rdf:resource="&fibo-sec-dbt-dbt-ins;NonTradableDebtInstrument"/>
      <rdfs:range rdf:resource="&fibo-sec-dbt-dbt-ins;IssuedDebt"/>
   </owl:ObjectProperty>

   <owl:ObjectProperty rdf:about="&fibo-sec-dbt-dbt-ins;mayBeSubordinatedTo">
      <rdfs:label>may be subordinated to</rdfs:label>
      <rdfs:domain rdf:resource="&fibo-sec-dbt-dbt-ins;TradableDebtInstrument"/>
      <rdfs:range rdf:resource="&fibo-sec-dbt-dbt-ins;TradableDebtInstrument"/>
   </owl:ObjectProperty>

   <owl:ObjectProperty rdf:about="&fibo-sec-dbt-dbt-ins;denomination">
      <rdfs:label>denomination</rdfs:label>
      <skos:definition>The face value of an individual note of the security.</skos:definition>
      <rdfs:domain rdf:resource="&fibo-sec-dbt-dbt-ins;TradableDebtInstrument"/>
      <rdfs:range rdf:resource="&fibo-fnd-acc-cur;MoneyAmount"/>
   </owl:ObjectProperty>

   <owl:ObjectProperty rdf:about="&fibo-sec-dbt-dbt-ins;setsOutTermsFor">
      <rdfs:label>sets out terms for</rdfs:label>
      <rdfs:domain rdf:resource="&fibo-sec-dbt-dbt-ins;TradableDebtInstrument"/>
      <rdfs:range rdf:resource="&fibo-sec-dbt-dbt-ins;PubliclyIssuedDebt"/>
   </owl:ObjectProperty>

   <owl:ObjectProperty rdf:about="&fibo-sec-dbt-dbt-ins;issuedDebtAmount">
      <rdfs:label>issued debt amount</rdfs:label>
      <skos:definition>The amount of Debt issued.</skos:definition>
      <rdfs:domain rdf:resource="&fibo-sec-dbt-dbt-ins;PubliclyIssuedDebt"/>
      <rdfs:range rdf:resource="&fibo-fnd-acc-cur;MoneyAmount"/>
   </owl:ObjectProperty>


  <!--
    ///////////////////////////////////////////////////////////////////////////////////////
    //
    // Data Properties
    //
    ///////////////////////////////////////////////////////////////////////////////////////
    -->


<owl:DatatypeProperty rdf:about="&fibo-sec-dbt-dbt-ins;callable">
      <rdfs:label>callable</rdfs:label>
      <skos:definition>Whether the writer of the debt contract (the debtor) can call the debt prior to maturity.</skos:definition>
      <rdfs:range rdf:resource="&fibo-fnd-utl-bt;yesOrNo"/>
   </owl:DatatypeProperty>

   <owl:DatatypeProperty rdf:about="&fibo-sec-dbt-dbt-ins;putable">
      <rdfs:label>putable</rdfs:label>
      <skos:definition>Whether the holder has the right to ask for redemption of the security prior to final maturity.</skos:definition>
      <rdfs:range rdf:resource="&fibo-fnd-utl-bt;yesOrNo"/>
   </owl:DatatypeProperty>

   <owl:DatatypeProperty rdf:about="&fibo-sec-dbt-dbt-ins;valueAtIssue">
      <rdfs:label>value at issue</rdfs:label>
      <skos:definition>The relative value at which the instrument is issued, namely par, premium or discount.</skos:definition>
      <rdfs:range rdf:resource="&fibo-sec-dbt-dbt-par;DebtRelativeValueSelection"/>
   </owl:DatatypeProperty>

   <owl:DatatypeProperty rdf:about="&fibo-sec-dbt-dbt-ins;valueAtMaturity">
      <rdfs:label>value at maturity</rdfs:label>
      <skos:definition>The value at which the instrument matures, namely par, discount or premium.</skos:definition>
      <rdfs:range rdf:resource="&fibo-sec-dbt-dbt-par;DebtRelativeValueSelection"/>
   </owl:DatatypeProperty>

   <owl:DatatypeProperty rdf:about="&fibo-sec-dbt-dbt-ins;callable.1">
      <rdfs:label>callable</rdfs:label>
      <skos:definition>Whether the issuer of the debt instrument can call the debt prior to maturity.</skos:definition>
      <rdfs:range rdf:resource="&fibo-fnd-utl-bt;yesOrNo"/>
   </owl:DatatypeProperty>

   <owl:DatatypeProperty rdf:about="&fibo-sec-dbt-dbt-ins;defaultLotSize">
      <rdfs:label>default lot size</rdfs:label>
      <skos:definition>The number of units of the security that may be held at any one time. This is the minimum denomination required for transfer or change of ownership of a tradable debt security.</skos:definition>
      <rdfs:range rdf:resource="&fibo-fnd-utl-bt;number"/>
   </owl:DatatypeProperty>

   <owl:DatatypeProperty rdf:about="&fibo-sec-dbt-dbt-ins;exchangeable">
      <rdfs:label>exchangeable</rdfs:label>
      <skos:definition>Whether the security can be exchanged for another security at the issuers discretion.</skos:definition>
      <rdfs:range rdf:resource="&fibo-fnd-utl-bt;yesOrNo"/>
   </owl:DatatypeProperty>

   <owl:DatatypeProperty rdf:about="&fibo-sec-dbt-dbt-ins;maturityDuration">
      <rdfs:label>maturity duration</rdfs:label>
      <skos:definition>Length of time of the life of the Tradable Debt Instrument in days, months and years. This is the duration from the issue date to the scheduled maturity date.</skos:definition>
      <rdfs:range rdf:resource="&fibo-fnd-tim-tim;KnownCalendarDuration"/>
   </owl:DatatypeProperty>

   <owl:DatatypeProperty rdf:about="&fibo-sec-dbt-dbt-ins;priceAndYieldDayCountConvention">
      <rdfs:label>price and yield day count convention</rdfs:label>
      <skos:definition>The number of days in a month and days in a year that are counted when performing calculations for yield and price figures.</skos:definition>
      <rdfs:range rdf:resource="&fibo-sec-dbt-dbt-ins;DayCountBasis"/>
   </owl:DatatypeProperty>

   <owl:DatatypeProperty rdf:about="&fibo-sec-dbt-dbt-ins;putable.1">
      <rdfs:label>putable</rdfs:label>
      <skos:definition>Whether the holder has the right to ask for redemption of the security prior to final maturity.</skos:definition>
      <rdfs:range rdf:resource="&fibo-fnd-utl-bt;yesOrNo"/>
   </owl:DatatypeProperty>

   <owl:DatatypeProperty rdf:about="&fibo-sec-dbt-dbt-ins;strippable">
      <rdfs:label>strippable</rdfs:label>
      <skos:definition>Whether or not the instrument can be stripped, so that interest and principal may be traded separately.</skos:definition>
      <rdfs:range rdf:resource="&fibo-fnd-utl-bt;yesOrNo"/>
   </owl:DatatypeProperty>

   <owl:DatatypeProperty rdf:about="&fibo-sec-dbt-dbt-ins;subordinated">
      <rdfs:label>subordinated</rdfs:label>
      <skos:definition>Whether the security is a subordinated security. This means that the security has a lower priority than another security so that when the assets are liquidated this one is not first in line.</skos:definition>
      <rdfs:range rdf:resource="&fibo-fnd-utl-bt;yesOrNo"/>
   </owl:DatatypeProperty>

   <owl:DatatypeProperty rdf:about="&fibo-sec-dbt-dbt-ins;valueAtIssue.1">
      <rdfs:label>value at issue</rdfs:label>
      <skos:definition>The relative value at which the instrument is issued, namely par, premium or discount.</skos:definition>
      <rdfs:range rdf:resource="&fibo-sec-dbt-dbt-par;DebtRelativeValueSelection"/>
   </owl:DatatypeProperty>

   <owl:DatatypeProperty rdf:about="&fibo-sec-dbt-dbt-ins;valueAtMaturity.1">
      <rdfs:label>value at maturity</rdfs:label>
      <skos:definition>The value at which the instrument matures, namely par, discount or premium.</skos:definition>
      <rdfs:range rdf:resource="&fibo-sec-dbt-dbt-par;DebtRelativeValueSelection"/>
   </owl:DatatypeProperty>

   <owl:DatatypeProperty rdf:about="&fibo-sec-dbt-dbt-ins;poolNumber">
      <rdfs:label>pool number</rdfs:label>
      <skos:definition>The Pool Number of the debt.</skos:definition>
      <rdfs:range rdf:resource="&fibo-fnd-utl-bt;wholeNumber"/>
   </owl:DatatypeProperty>

   <owl:DatatypeProperty rdf:about="&fibo-sec-dbt-dbt-ins;series">
      <rdfs:label>series</rdfs:label>
      <skos:definition>A series number, identified by the issuer in the event that debt is issued in several series (also known as tranches).</skos:definition>
      <rdfs:range rdf:resource="&fibo-fnd-utl-bt;text"/>
   </owl:DatatypeProperty>


  <!--
    ///////////////////////////////////////////////////////////////////////////////////////
    //
    // Annotation Properties
    //
    ///////////////////////////////////////////////////////////////////////////////////////
    -->



  <!--
    ///////////////////////////////////////////////////////////////////////////////////////
    //
    // Classes
    //
    ///////////////////////////////////////////////////////////////////////////////////////
    -->


<owl:Class rdf:about="&fibo-sec-dbt-dbt-ins;.UnionClass.7">
      <skos:definition>A paper or electronic obligation that enables the issuing party to raise funds by promising to repay a lender in accordance with terms of a contract. Types of debt instruments include notes, bonds, certificates, mortgages, leases or other agreements between a lender and a borrower.</skos:definition>
      <owl:equivalentClass>
         <owl:Class>
            <owl:unionOf rdf:parseType="Collection">
               <owl:Class rdf:about="&fibo-sec-dbt-dbt-ins;NonTradableDebtInstrument"/>
               <owl:Class rdf:about="&fibo-sec-dbt-mm-tr;.UnionClass.68"/>
               <owl:Class rdf:about="&fibo-sec-dbt-mm-repo;RepurchaseAgreement"/>
               <owl:Class rdf:about="&fibo-sec-dbt-dbt-ins;TradableDebtInstrument"/>
            </owl:unionOf>
         </owl:Class>
      </owl:equivalentClass>
   </owl:Class>

   <owl:Class rdf:about="&fibo-sec-dbt-dbt-ins;IssuedDebt">
      <rdfs:label>issued debt</rdfs:label>
      <skos:definition>Debt which is set out by the borrower in some form of financial security in which the lender is the holder or counterparty of that security.</skos:definition>
      <rdfs:subClassOf rdf:resource="&fibo-fnd-acc-dbt;DebtFinance"/>
   </owl:Class>

   <owl:Class rdf:about="&fibo-sec-dbt-dbt-ins;NonTradableDebtInstrument">
      <rdfs:label>non tradable debt instrument</rdfs:label>
      <rdfs:subClassOf rdf:resource="&fibo-fnd-agr-ctr;BilateralContract"/>
   </owl:Class>

   <owl:Class rdf:about="&fibo-sec-dbt-dbt-ins;TradableDebtInstrument">
      <rdfs:label>tradable debt instrument</rdfs:label>
      <skos:definition>A debt instrument which can be bought and sold by the holder. This typically has a security identifier.</skos:definition>
      <rdfs:subClassOf rdf:resource="&fibo-sec-sec-sec;Security"/>
   </owl:Class>

   <owl:Class rdf:about="&fibo-sec-dbt-dbt-ins;PubliclyIssuedDebt">
      <rdfs:label>publicly issued debt</rdfs:label>
      <skos:definition>An amount of Debt issued under a given Debt security.</skos:definition>
      <rdfs:subClassOf rdf:resource="&fibo-sec-dbt-dbt-ins;IssuedDebt"/>
   </owl:Class>


  <!--
    ///////////////////////////////////////////////////////////////////////////////////////
    //
    // Individuals
    //
    ///////////////////////////////////////////////////////////////////////////////////////
    -->


</rdf:RDF>