<?xml version="1.0" encoding="UTF-8"?>
<rdf:RDF xmlns:xsd="http://www.w3.org/2001/XMLSchema#"
         xmlns:sm="http://www.omg.org/techprocess/ab/SpecificationMetadata/"
         xmlns:fibo-fnd-utl-av="http://www.omg.org/spec/EDMC-FIBO/FND/Utilities/AnnotationVocabulary/"
         xmlns:rdf="http://www.w3.org/1999/02/22-rdf-syntax-ns#"
         xmlns:rdfs="http://www.w3.org/2000/01/rdf-schema#"
         xmlns:owl="http://www.w3.org/2002/07/owl#"
         xmlns:skos="http://www.w3.org/2004/02/skos/core#"
         xmlns:dc="http://purl.org/dc/terms/"
         xml:base="http://www.edmcouncil.org/spec/EDMC-SR/FND/AgreementsExt/ContractsIllustrative/">

   <owl:Ontology rdf:about="http://www.edmcouncil.org/spec/EDMC-SR/FND/AgreementsExt/ContractsIllustrative/">
      <owl:imports rdf:resource="http://www.omg.org/spec/EDMC-SR/FND/Agreements/Contracts/"/>
   </owl:Ontology>

   <!--Datatypes-->

<!--Object Properties-->

<owl:ObjectProperty rdf:about="http://www.edmcouncil.org/spec/EDMC-SR/FND/AgreementsExt/ContractsIllustrative/heldBy">
      <skos:definition>The party which holds the license and enjoys the rights and benefits described in the license agreement.</skos:definition>
      <rdfs:subPropertyOf rdf:resource="http://www.omg.org/spec/EDMC-SR/FND/Agreements/Contracts/heldBy"/>
      <rdfs:domain rdf:resource="http://www.edmcouncil.org/spec/EDMC-SR/FND/AgreementsExt/ContractsIllustrative/License"/>
      <rdfs:range rdf:resource="http://www.edmcouncil.org/spec/EDMC-SR/FND/AgreementsExt/ContractsIllustrative/Licensee"/>
   </owl:ObjectProperty>

   <owl:ObjectProperty rdf:about="http://www.edmcouncil.org/spec/EDMC-SR/FND/AgreementsExt/ContractsIllustrative/issuedBy">
      <skos:definition>The party which issues the license and extends the rights defined in the license agreement.</skos:definition>
      <rdfs:subPropertyOf rdf:resource="http://www.omg.org/spec/EDMC-SR/FND/Agreements/Contracts/writtenBy"/>
      <rdfs:domain rdf:resource="http://www.edmcouncil.org/spec/EDMC-SR/FND/AgreementsExt/ContractsIllustrative/License"/>
      <rdfs:range rdf:resource="http://www.edmcouncil.org/spec/EDMC-SR/FND/AgreementsExt/ContractsIllustrative/Licensor"/>
   </owl:ObjectProperty>

   <!--Data Properties-->

<!--Annotation Properties-->

<!--Classes-->

<owl:Class rdf:about="http://www.edmcouncil.org/spec/EDMC-SR/FND/AgreementsExt/ContractsIllustrative/License">
      <rdfs:label>License</rdfs:label>
      <skos:definition>A contract conferring certain rights and obligations on the holder of the contract (the licensee) who is generally unknown to the license issuer (the licensor).</skos:definition>
      <skos:editorialNote>A License may be transferred by the licensee (holder) to another party that becomes the new licensee without reference to the licensor. A software license is a kind of license in this sense.</skos:editorialNote>
      <rdfs:subClassOf rdf:resource="http://www.omg.org/spec/EDMC-SR/FND/Agreements/Contracts/TransferableContract"/>
   </owl:Class>

   <owl:Class rdf:about="http://www.edmcouncil.org/spec/EDMC-SR/FND/AgreementsExt/ContractsIllustrative/Licensee">
      <rdfs:label>Licensee</rdfs:label>
      <skos:definition>The holder of a license such as a software license.</skos:definition>
      <rdfs:subClassOf rdf:resource="http://www.omg.org/spec/EDMC-SR/FND/Agreements/Contracts/TransferableContractHolder"/>
   </owl:Class>

   <owl:Class rdf:about="http://www.edmcouncil.org/spec/EDMC-SR/FND/AgreementsExt/ContractsIllustrative/Licensor">
      <rdfs:label>Licensor</rdfs:label>
      <skos:definition>The issuer of a license such as a software llicense.</skos:definition>
      <rdfs:subClassOf rdf:resource="http://www.omg.org/spec/EDMC-SR/FND/Agreements/Contracts/ContractOriginator"/>
   </owl:Class>

   <owl:Class rdf:about="http://www.edmcouncil.org/spec/EDMC-SR/FND/AgreementsExt/ContractsIllustrative/SoftwareLicense">
      <rdfs:label>Software License</rdfs:label>
      <rdfs:subClassOf rdf:resource="http://www.edmcouncil.org/spec/EDMC-SR/FND/AgreementsExt/ContractsIllustrative/License"/>
   </owl:Class>

   <!--Individuals-->

</rdf:RDF>