<?xml version="1.0" encoding="UTF-8"?>
  
<!DOCTYPE rdf:RDF [
    <!ENTITY fibo-der-etd-ox "http://spec.edmcouncil.org/fibo/red/der/exchange-traded-derivatives/options-exchanges/">
    <!ENTITY fibo-fnd-acc-acc "http://spec.edmcouncil.org/fibo/red/fnd/accounting/accounting-main/">
    <!ENTITY fibo-der-etd-dst "http://spec.edmcouncil.org/fibo/red/der/exchange-traded-derivatives/derivatives-standardized-terms/">
    <!ENTITY fibo-fnd-pty-pty "http://spec.edmcouncil.org/fibo/red/fnd/parties/parties/">
]>

<rdf:RDF xmlns:xsd="http://www.w3.org/2001/XMLSchema#"
         xmlns:sm="http://www.omg.org/techprocess/ab/SpecificationMetadata/"
         xmlns:xs="http://www.w3.org/2001/XMLSchema"
         xmlns:fibo-fnd-utl-av="http://www.omg.org/spec/EDMC-FIBO/FND/Utilities/AnnotationVocabulary/"
         xmlns:rdf="http://www.w3.org/1999/02/22-rdf-syntax-ns#"
         xmlns:rdfs="http://www.w3.org/2000/01/rdf-schema#"
         xmlns:owl="http://www.w3.org/2002/07/owl#"
         xmlns:skos="http://www.w3.org/2004/02/skos/core#"
         xmlns:dc="http://purl.org/dc/terms/"
         xml:base="http://spec.edmcouncil.org/fibo/red/der/exchange-traded-derivatives/options-exchanges/">

   <owl:Ontology rdf:about="http://spec.edmcouncil.org/fibo/red/der/exchange-traded-derivatives/options-exchanges/">
      <owl:imports rdf:resource="http://spec.edmcouncil.org/fibo/red/fnd/accounting/accounting-main/"/>
      <owl:imports rdf:resource="http://spec.edmcouncil.org/fibo/red/der/exchange-traded-derivatives/derivatives-standardized-terms/"/>
      <owl:imports rdf:resource="http://spec.edmcouncil.org/fibo/red/fnd/parties/parties/"/>
   </owl:Ontology>


  <!--
    ///////////////////////////////////////////////////////////////////////////////////////
    //
    // Datatypes
    //
    ///////////////////////////////////////////////////////////////////////////////////////
    -->



  <!--
    ///////////////////////////////////////////////////////////////////////////////////////
    //
    // Object Properties
    //
    ///////////////////////////////////////////////////////////////////////////////////////
    -->


<owl:ObjectProperty rdf:about="&fibo-der-etd-ox;canBecome">
      <rdfs:label>can become</rdfs:label>
      <rdfs:domain rdf:resource="&fibo-der-etd-ox;TradingParticipant"/>
      <rdfs:range rdf:resource="&fibo-der-etd-ox;ClearingParticipant"/>
   </owl:ObjectProperty>

   <owl:ObjectProperty rdf:about="&fibo-der-etd-ox;mayBe">
      <rdfs:label>may be</rdfs:label>
      <rdfs:domain rdf:resource="&fibo-der-etd-ox;TradingParticipant"/>
      <rdfs:range rdf:resource="&fibo-der-etd-ox;DerivativesBroker"/>
   </owl:ObjectProperty>


  <!--
    ///////////////////////////////////////////////////////////////////////////////////////
    //
    // Data Properties
    //
    ///////////////////////////////////////////////////////////////////////////////////////
    -->



  <!--
    ///////////////////////////////////////////////////////////////////////////////////////
    //
    // Annotation Properties
    //
    ///////////////////////////////////////////////////////////////////////////////////////
    -->



  <!--
    ///////////////////////////////////////////////////////////////////////////////////////
    //
    // Classes
    //
    ///////////////////////////////////////////////////////////////////////////////////////
    -->


<owl:Class rdf:about="&fibo-der-etd-ox;ClearingParticipant">
      <rdfs:label>clearing participant</rdfs:label>
      <skos:definition>People who are members of the exchange who are allowed to clear the trades. There are various categories of entities which are participating in this full process: FTrading Member Clearing Member Entity which does both for itself (not professionally carrying out the clearing for other</skos:definition>
      <rdfs:subClassOf rdf:resource="&fibo-der-etd-ox;TradingParticipant"/>
   </owl:Class>

   <owl:Class rdf:about="&fibo-der-etd-ox;DerivativesBroker">
      <rdfs:label>derivatives broker</rdfs:label>
      <skos:definition>A party which is party to the transaction between entities which are not on the Derivatives Exchange. The Broker is then also a member of the Exchange (see Trading PArticipant), and in this context is the one who carries out the deals on the exchange, and who settles his margin daily. These may poarticipate in the OTC market also, where they just get a fee for introdiucing them. In formal exchanges, the Broker is doing th edeal, and the fact that the deal is passed on to others is a separate transaction, which they are also party to.</skos:definition>
   </owl:Class>

   <owl:Class rdf:about="&fibo-der-etd-ox;MarginAccount">
      <rdfs:label>margin account</rdfs:label>
      <skos:definition>Account held at a Derivatives Exchange by a participant in that exchange.</skos:definition>
      <rdfs:subClassOf rdf:resource="&fibo-fnd-acc-acc;Account"/>
   </owl:Class>

   <owl:Class rdf:about="&fibo-der-etd-ox;OptionsExchangeParticipant">
      <rdfs:label>options exchange participant</rdfs:label>
      <rdfs:subClassOf rdf:resource="&fibo-fnd-pty-pty;PartyInRole"/>
   </owl:Class>

   <owl:Class rdf:about="&fibo-der-etd-ox;OptionsListing">
      <rdfs:label>options listing</rdfs:label>
      <skos:definition>A listing of an options instrument on a derivatives exchange. The listing is a product of the individual exchange.</skos:definition>
      <rdfs:subClassOf rdf:resource="&fibo-der-etd-dst;DerivativesListing"/>
   </owl:Class>

   <owl:Class rdf:about="&fibo-der-etd-ox;TradingParticipant">
      <rdfs:label>trading participant</rdfs:label>
      <rdfs:subClassOf rdf:resource="&fibo-der-etd-ox;OptionsExchangeParticipant"/>
   </owl:Class>


  <!--
    ///////////////////////////////////////////////////////////////////////////////////////
    //
    // Individuals
    //
    ///////////////////////////////////////////////////////////////////////////////////////
    -->


</rdf:RDF>