<?xml version="1.0" encoding="UTF-8"?>
  
<!DOCTYPE rdf:RDF [
    <!ENTITY fibo-der-etd-ost "http://spec.edmcouncil.org/fibo/red/der/exchange-traded-derivatives/options-standardized-terms/">
    <!ENTITY fibo-fnd-bus-pol "http://spec.edmcouncil.org/fibo/red/fnd/business/policy/">
    <!ENTITY fibo-be-le-fbo "http://spec.edmcouncil.org/fibo/red/be/legal-entities/formal-business-organizations/">
    <!ENTITY fibo-sec-sec-ctr "http://spec.edmcouncil.org/fibo/red/sec/securities/instrument-contracts/">
    <!ENTITY fibo-fnd-utl-bt "http://spec.edmcouncil.org/fibo/red/fnd/utilities/business-facing-types/">
    <!ENTITY fibo-fnd-pub-pub "http://spec.edmcouncil.org/fibo/red/fnd/publications/publications/">
    <!ENTITY fibo-sec-sec-fi "http://spec.edmcouncil.org/fibo/red/sec/securities/financial-instruments/">
    <!ENTITY fibo-der-ctr-opt "http://spec.edmcouncil.org/fibo/red/der/derivatives-contracts/options/">
    <!ENTITY fibo-der-etd-opt "http://spec.edmcouncil.org/fibo/red/der/exchange-traded-derivatives/exchange-traded-options/">
    <!ENTITY fibo-der-etd-dst "http://spec.edmcouncil.org/fibo/red/der/exchange-traded-derivatives/derivatives-standardized-terms/">
    <!ENTITY fibo-fnd-acc-cur "http://spec.edmcouncil.org/fibo/red/fnd/accounting/currency-amount/">
]>

<rdf:RDF xmlns:xsd="http://www.w3.org/2001/XMLSchema#"
         xmlns:sm="http://www.omg.org/techprocess/ab/SpecificationMetadata/"
         xmlns:xs="http://www.w3.org/2001/XMLSchema"
         xmlns:fibo-fnd-utl-av="http://www.omg.org/spec/EDMC-FIBO/FND/Utilities/AnnotationVocabulary/"
         xmlns:rdf="http://www.w3.org/1999/02/22-rdf-syntax-ns#"
         xmlns:rdfs="http://www.w3.org/2000/01/rdf-schema#"
         xmlns:owl="http://www.w3.org/2002/07/owl#"
         xmlns:skos="http://www.w3.org/2004/02/skos/core#"
         xmlns:dc="http://purl.org/dc/terms/"
         xml:base="http://spec.edmcouncil.org/fibo/red/der/exchange-traded-derivatives/options-standardized-terms/">

   <owl:Ontology rdf:about="http://spec.edmcouncil.org/fibo/red/der/exchange-traded-derivatives/options-standardized-terms/">
      <owl:imports rdf:resource="http://spec.edmcouncil.org/fibo/red/fnd/business/policy/"/>
      <owl:imports rdf:resource="http://spec.edmcouncil.org/fibo/red/be/legal-entities/formal-business-organizations/"/>
      <owl:imports rdf:resource="http://spec.edmcouncil.org/fibo/red/sec/securities/instrument-contracts/"/>
      <owl:imports rdf:resource="http://spec.edmcouncil.org/fibo/red/fnd/utilities/business-facing-types/"/>
      <owl:imports rdf:resource="http://spec.edmcouncil.org/fibo/red/fnd/publications/publications/"/>
      <owl:imports rdf:resource="http://spec.edmcouncil.org/fibo/red/sec/securities/financial-instruments/"/>
      <owl:imports rdf:resource="http://spec.edmcouncil.org/fibo/red/der/derivatives-contracts/options/"/>
      <owl:imports rdf:resource="http://spec.edmcouncil.org/fibo/red/der/exchange-traded-derivatives/exchange-traded-options/"/>
      <owl:imports rdf:resource="http://spec.edmcouncil.org/fibo/red/der/exchange-traded-derivatives/derivatives-standardized-terms/"/>
      <owl:imports rdf:resource="http://spec.edmcouncil.org/fibo/red/fnd/accounting/currency-amount/"/>
   </owl:Ontology>


  <!--
    ///////////////////////////////////////////////////////////////////////////////////////
    //
    // Datatypes
    //
    ///////////////////////////////////////////////////////////////////////////////////////
    -->



  <!--
    ///////////////////////////////////////////////////////////////////////////////////////
    //
    // Object Properties
    //
    ///////////////////////////////////////////////////////////////////////////////////////
    -->


<owl:ObjectProperty rdf:about="&fibo-der-etd-ost;specifies">
      <rdfs:label>specifies</rdfs:label>
      <rdfs:domain rdf:resource="&fibo-der-etd-ost;StandardizedExerciseTermsSet"/>
      <rdfs:range rdf:resource="&fibo-sec-sec-fi;FinancialInstrument"/>
   </owl:ObjectProperty>

   <owl:ObjectProperty rdf:about="&fibo-der-etd-ost;pricingToBeDeterminedBy">
      <rdfs:label>pricing to be determined by</rdfs:label>
      <rdfs:domain rdf:resource="&fibo-der-etd-ost;StandardizedOptionsTermsSet"/>
      <rdfs:range rdf:resource="&fibo-der-etd-ost;OptionPriceDeterminationMethod"/>
   </owl:ObjectProperty>

   <owl:ObjectProperty rdf:about="&fibo-der-etd-ost;becomesTermsOf">
      <rdfs:label>becomes terms of</rdfs:label>
      <rdfs:domain rdf:resource="&fibo-der-etd-ost;StandardizedOptionsTermsSet"/>
      <rdfs:range rdf:resource="&fibo-der-etd-opt;ExchangeTradedOptionContract"/>
   </owl:ObjectProperty>

   <owl:ObjectProperty rdf:about="&fibo-der-etd-ost;includesFeature">
      <rdfs:label>includes feature</rdfs:label>
      <rdfs:domain rdf:resource="&fibo-der-etd-ost;StandardizedOptionsTermsSet"/>
      <rdfs:range rdf:resource="&fibo-der-ctr-opt;OptionBarrierFeatureTerms"/>
   </owl:ObjectProperty>

   <owl:ObjectProperty rdf:about="&fibo-der-etd-ost;definedBy">
      <rdfs:label>defined by</rdfs:label>
      <rdfs:subPropertyOf rdf:resource="&fibo-fnd-pub-pub;publishedBy"/>
      <rdfs:domain rdf:resource="&fibo-der-etd-ost;StandardizedOptionsTermsSet"/>
      <rdfs:range rdf:resource="&fibo-der-etd-dst;.UnionClass.3"/>
   </owl:ObjectProperty>


  <!--
    ///////////////////////////////////////////////////////////////////////////////////////
    //
    // Data Properties
    //
    ///////////////////////////////////////////////////////////////////////////////////////
    -->


<owl:DatatypeProperty rdf:about="&fibo-der-etd-ost;priceDeterminationMethod">
      <rdfs:label>price determination method</rdfs:label>
      <skos:definition>The method by which the price is determined, for example open outcry.</skos:definition>
      <rdfs:range rdf:resource="&fibo-der-etd-dst;DerivativesPriceDeterminationMethodSelection"/>
   </owl:DatatypeProperty>

   <owl:DatatypeProperty rdf:about="&fibo-der-etd-ost;contractSize">
      <rdfs:label>contract size</rdfs:label>
      <skos:definition>The number of units of the currency traded under one Futures Contract.</skos:definition>
      <rdfs:range rdf:resource="&fibo-fnd-acc-cur;MoneyAmount"/>
   </owl:DatatypeProperty>

   <owl:DatatypeProperty rdf:about="&fibo-der-etd-ost;contractSize.1">
      <rdfs:label>contract size</rdfs:label>
      <skos:definition>The number of shares traded under one Option Contract.</skos:definition>
      <rdfs:range rdf:resource="&fibo-fnd-utl-bt;wholeNumber"/>
   </owl:DatatypeProperty>

   <owl:DatatypeProperty rdf:about="&fibo-der-etd-ost;contractSize.2">
      <rdfs:label>contract size</rdfs:label>
      <skos:definition>The number of futures contracts traded under one Futures Option.</skos:definition>
      <rdfs:range rdf:resource="&fibo-fnd-utl-bt;wholeNumber"/>
   </owl:DatatypeProperty>

   <owl:DatatypeProperty rdf:about="&fibo-der-etd-ost;indexMultiplier">
      <rdfs:label>index multiplier</rdfs:label>
      <skos:definition>The multiple of the index traded under one Futures contract.</skos:definition>
      <rdfs:range rdf:resource="&fibo-fnd-utl-bt;number"/>
   </owl:DatatypeProperty>

   <owl:DatatypeProperty rdf:about="&fibo-der-etd-ost;contractSize.3">
      <rdfs:label>contract size</rdfs:label>
      <skos:definition>Number of underlyers to be in a contract.</skos:definition>
      <rdfs:range rdf:resource="&fibo-fnd-utl-bt;wholeNumber"/>
   </owl:DatatypeProperty>

   <owl:DatatypeProperty rdf:about="&fibo-der-etd-ost;optionType">
      <rdfs:label>option type</rdfs:label>
      <skos:definition>Whether the option will be a call or a put option.</skos:definition>
      <rdfs:range rdf:resource="&fibo-der-ctr-opt;OptionTypeSelection"/>
   </owl:DatatypeProperty>


  <!--
    ///////////////////////////////////////////////////////////////////////////////////////
    //
    // Annotation Properties
    //
    ///////////////////////////////////////////////////////////////////////////////////////
    -->



  <!--
    ///////////////////////////////////////////////////////////////////////////////////////
    //
    // Classes
    //
    ///////////////////////////////////////////////////////////////////////////////////////
    -->


<owl:Class rdf:about="&fibo-der-etd-ost;OptionPriceDeterminationMethod">
      <rdfs:label>option price determination method</rdfs:label>
      <skos:definition>The method by which the price of a traded option instrument is to be determined.</skos:definition>
      <rdfs:subClassOf rdf:resource="&fibo-fnd-bus-pol;Method"/>
   </owl:Class>

   <owl:Class rdf:about="&fibo-der-etd-ost;OptionsClearingEntity">
      <rdfs:label>options clearing entity</rdfs:label>
      <skos:definition>An entity which is responsible for clearing transactions for put and call options on common stocks and other equity issues, stock indexes, foreign currencies, interest rate composites and single-stock futures.</skos:definition>
      <rdfs:subClassOf rdf:resource="&fibo-be-le-fbo;FormallyConstitutedOrganization"/>
   </owl:Class>

   <owl:Class rdf:about="&fibo-der-etd-ost;StandardizedCurrencyOptionTermsSet">
      <rdfs:label>standardized currency option terms set</rdfs:label>
      <skos:definition>Standard terms for a currency optioon contract, determined in advance by the exchange. These will become terms of an individual currency option contract. These may be varied or overridden for individual contracts.</skos:definition>
      <rdfs:subClassOf rdf:resource="&fibo-der-etd-ost;StandardizedOptionsTermsSet"/>
   </owl:Class>

   <owl:Class rdf:about="&fibo-der-etd-ost;StandardizedEquityOptionTermsSet">
      <rdfs:label>standardized equity option terms set</rdfs:label>
      <skos:definition>Standard terms for an equity option contract, determined in advance by the exchange. These will become terms of an individual equity option contract. These may be varied or overridden for individual contracts.</skos:definition>
   </owl:Class>

   <owl:Class rdf:about="&fibo-der-etd-ost;StandardizedExerciseTermsSet">
      <rdfs:label>standardized exercise terms set</rdfs:label>
      <skos:definition>Standard exercise terms for an option contract, determined in advance by the exchange. These will become exercise terms of an individual option contract. These may be varied or overridden for individual contracts.</skos:definition>
   </owl:Class>

   <owl:Class rdf:about="&fibo-der-etd-ost;StandardizedFuturesOptionTermsSet">
      <rdfs:label>standardized futures option terms set</rdfs:label>
      <skos:definition>Standard terms for a futures options contract, determined in advance by the exchange. These will become terms of an individual futures option contract. These may be varied or overridden for individual contracts.</skos:definition>
   </owl:Class>

   <owl:Class rdf:about="&fibo-der-etd-ost;StandardizedIndexOptionTermsSet">
      <rdfs:label>standardized index option terms set</rdfs:label>
      <skos:definition>Standard terms for an index option contract, determined in advance by the exchange. These will become terms of an individual index option contract. These may be varied or overridden for individual contracts.</skos:definition>
   </owl:Class>

   <owl:Class rdf:about="&fibo-der-etd-ost;StandardizedOptionsTermsSet">
      <rdfs:label>standardized options terms set</rdfs:label>
      <skos:definition>A standardized set of terms for an options contract. These are defined by a securities exchange or an options clearing entity. Options contracts issued by the exchange may embody these terms or have equivalent terms which override these.</skos:definition>
      <rdfs:subClassOf rdf:resource="&fibo-sec-sec-ctr;StandardizedTermsSet"/>
   </owl:Class>


  <!--
    ///////////////////////////////////////////////////////////////////////////////////////
    //
    // Individuals
    //
    ///////////////////////////////////////////////////////////////////////////////////////
    -->


</rdf:RDF>