<?xml version="1.0" encoding="UTF-8"?>
  
<!DOCTYPE rdf:RDF [
    <!ENTITY fibo-be-fct-spv "http://spec.edmcouncil.org/fibo/red/be/functional-entities-ext/spv/">
    <!ENTITY fibo-be-fct-fct "http://spec.edmcouncil.org/fibo/red/be/functional-entities/functional-entities/">
    <!ENTITY fibo-be-le-fbo "http://spec.edmcouncil.org/fibo/red/be/legal-entities/formal-business-organizations/">
    <!ENTITY fibo-be-le-lp "http://spec.edmcouncil.org/fibo/red/be/legal-entities/legal-persons/">
]>

<rdf:RDF xmlns:xsd="http://www.w3.org/2001/XMLSchema#"
         xmlns:sm="http://www.omg.org/techprocess/ab/SpecificationMetadata/"
         xmlns:xs="http://www.w3.org/2001/XMLSchema"
         xmlns:fibo-fnd-utl-av="http://www.omg.org/spec/EDMC-FIBO/FND/Utilities/AnnotationVocabulary/"
         xmlns:rdf="http://www.w3.org/1999/02/22-rdf-syntax-ns#"
         xmlns:rdfs="http://www.w3.org/2000/01/rdf-schema#"
         xmlns:owl="http://www.w3.org/2002/07/owl#"
         xmlns:skos="http://www.w3.org/2004/02/skos/core#"
         xmlns:dc="http://purl.org/dc/terms/"
         xml:base="http://spec.edmcouncil.org/fibo/red/be/functional-entities-ext/spv/">

   <owl:Ontology rdf:about="http://spec.edmcouncil.org/fibo/red/be/functional-entities-ext/spv/">
      <owl:imports rdf:resource="http://spec.edmcouncil.org/fibo/red/be/functional-entities/functional-entities/"/>
      <owl:imports rdf:resource="http://spec.edmcouncil.org/fibo/red/be/legal-entities/formal-business-organizations/"/>
      <owl:imports rdf:resource="http://spec.edmcouncil.org/fibo/red/be/legal-entities/legal-persons/"/>
   </owl:Ontology>


  <!--
    ///////////////////////////////////////////////////////////////////////////////////////
    //
    // Datatypes
    //
    ///////////////////////////////////////////////////////////////////////////////////////
    -->


<rdfs:Datatype rdf:about="&fibo-be-fct-spv;SPVPurposeSelection">
      <skos:definition>The reason that an SPV was set up.</skos:definition>
      <owl:equivalentClass>
         <rdfs:Datatype>
            <owl:oneOf>
               <rdf:Description>
                  <rdf:first rdf:datatype="http://www.w3.org/2001/XMLSchema#string">Debt</rdf:first>
                  <rdf:rest>
                     <rdf:Description>
                        <rdf:first rdf:datatype="http://www.w3.org/2001/XMLSchema#string">Securities Issuance</rdf:first>
                        <rdf:rest>
                           <rdf:Description>
                              <rdf:first rdf:datatype="http://www.w3.org/2001/XMLSchema#string">Fund</rdf:first>
                              <rdf:rest rdf:resource="http://www.w3.org/1999/02/22-rdf-syntax-ns#nil"/>
                           </rdf:Description>
                        </rdf:rest>
                     </rdf:Description>
                  </rdf:rest>
               </rdf:Description>
            </owl:oneOf>
         </rdfs:Datatype>
      </owl:equivalentClass>
   </rdfs:Datatype>


  <!--
    ///////////////////////////////////////////////////////////////////////////////////////
    //
    // Object Properties
    //
    ///////////////////////////////////////////////////////////////////////////////////////
    -->


<owl:ObjectProperty rdf:about="&fibo-be-fct-spv;constitutedAs">
      <rdfs:label>constituted as</rdfs:label>
      <skos:definition>The Special Purpose Vehicle is constituted as some kind of Formal Organization.</skos:definition>
      <rdfs:subPropertyOf rdf:resource="&fibo-be-fct-fct;functionalBusinessEntityTakesForm"/>
      <rdfs:domain rdf:resource="&fibo-be-fct-spv;SpecialPurposeVehicle"/>
      <rdfs:range rdf:resource="&fibo-be-le-fbo;FormallyConstitutedOrganization"/>
   </owl:ObjectProperty>

   <owl:ObjectProperty rdf:about="&fibo-be-fct-spv;sponsoredBy">
      <rdfs:label>sponsored by</rdfs:label>
      <skos:definition>The entity which is the creator and servicer of the SPV. Notes: To protect investors from possible bankruptcy of the corporation, there are three legal safeguards: - Transfer of assets from the corporation is a non-recourse, true sale. - Investors receive a perfected interest in the assets' cash flows. - A non-consolidation legal opinion is obtained certifying that assets of the trust or special purpose vehicle cannot be consolidated with the corporation's assets in the event of bankruptcy.</skos:definition>
      <rdfs:domain rdf:resource="&fibo-be-fct-spv;SpecialPurposeVehicle"/>
      <rdfs:range rdf:resource="&fibo-be-le-lp;LegalPerson"/>
   </owl:ObjectProperty>


  <!--
    ///////////////////////////////////////////////////////////////////////////////////////
    //
    // Data Properties
    //
    ///////////////////////////////////////////////////////////////////////////////////////
    -->


<owl:DatatypeProperty rdf:about="&fibo-be-fct-spv;intendedLiquidationDate">
      <rdfs:label>intended liquidation date</rdfs:label>
      <skos:definition>The date on which the SPV is scheduled to be disbanded and wound up.</skos:definition>
      <rdfs:range rdf:resource="http://www.w3.org/2001/XMLSchema#date"/>
   </owl:DatatypeProperty>

   <owl:DatatypeProperty rdf:about="&fibo-be-fct-spv;purpose">
      <rdfs:label>purpose</rdfs:label>
      <skos:definition>The purpose for which the SPV is set up.</skos:definition>
      <rdfs:range rdf:resource="&fibo-be-fct-spv;SPVPurposeSelection"/>
   </owl:DatatypeProperty>


  <!--
    ///////////////////////////////////////////////////////////////////////////////////////
    //
    // Annotation Properties
    //
    ///////////////////////////////////////////////////////////////////////////////////////
    -->



  <!--
    ///////////////////////////////////////////////////////////////////////////////////////
    //
    // Classes
    //
    ///////////////////////////////////////////////////////////////////////////////////////
    -->


<owl:Class rdf:about="&fibo-be-fct-spv;SpecialPurposeVehicle">
      <rdfs:label>special purpose vehicle</rdfs:label>
      <skos:definition>A Special Purpose Vehicle (SPV) set up specifically to issue a security or securities. It is set up by a company or a group of companies for some purpose such as to create instruments that are off the company's balance sheet or to issue Participation Notes for investors in another jurisdiction. The SPV is formed for a specific reason and exists for a specific period of time and is then disbanded. Further notes: Special Purpose Vehicles are also referred to as bankruptcy remote entities, as they isolate financial risk. For Participation Notes: slightly different purpose but the same kind of vehicle. The only investment made by the SPV is that they buy in the stock. These are the same kind of entity in all of the contexts in which they exist.</skos:definition>
      <rdfs:subClassOf rdf:resource="&fibo-be-fct-fct;FunctionalBusinessEntity"/>
   </owl:Class>


  <!--
    ///////////////////////////////////////////////////////////////////////////////////////
    //
    // Individuals
    //
    ///////////////////////////////////////////////////////////////////////////////////////
    -->


</rdf:RDF>