<?xml version="1.0" encoding="UTF-8"?>
<rdf:RDF xmlns:xsd="http://www.w3.org/2001/XMLSchema#"
         xmlns:sm="http://www.omg.org/techprocess/ab/SpecificationMetadata/"
         xmlns:fibo-fnd-utl-av="http://www.omg.org/spec/EDMC-FIBO/FND/Utilities/AnnotationVocabulary/"
         xmlns:rdf="http://www.w3.org/1999/02/22-rdf-syntax-ns#"
         xmlns:rdfs="http://www.w3.org/2000/01/rdf-schema#"
         xmlns:owl="http://www.w3.org/2002/07/owl#"
         xmlns:skos="http://www.w3.org/2004/02/skos/core#"
         xmlns:dc="http://purl.org/dc/terms/"
         xml:base="http://www.omg.org/spec/EDMC-SR/FND/Organizations/Organizations/">

   <owl:Ontology rdf:about="http://www.omg.org/spec/EDMC-SR/FND/Organizations/Organizations/">
      <owl:imports rdf:resource="http://www.omg.org/spec/EDMC-SR/FND/GoalsAndObjectives/Goals/"/>
      <owl:imports rdf:resource="http://www.omg.org/spec/EDMC-SR/FND/AgentsAndPeople/Agents/"/>
   </owl:Ontology>

   <!--Datatypes-->

<!--Object Properties-->

<owl:ObjectProperty rdf:about="http://www.omg.org/spec/EDMC-SR/FND/Organizations/Organizations/hasGoal">
      <skos:definition>The goal or objective for which the Organization was set up and which is the reason for its existence. This may be to make a profit for shareholders, to discharge the responsibilities of a Government, to propagate a faith or political purpose etc.</skos:definition>
      <rdfs:domain rdf:resource="http://www.omg.org/spec/EDMC-SR/FND/Organizations/Organizations/Organization"/>
      <rdfs:range rdf:resource="http://www.omg.org/spec/EDMC-SR/FND/GoalsAndObjectives/Goals/Goal"/>
   </owl:ObjectProperty>

   <owl:ObjectProperty rdf:about="http://www.omg.org/spec/EDMC-SR/FND/Organizations/Organizations/organizationHasMember">
      <skos:definition>The individuals that make up the organization.</skos:definition>
      <rdfs:domain rdf:resource="http://www.omg.org/spec/EDMC-SR/FND/Organizations/Organizations/Organization"/>
      <rdfs:range rdf:resource="http://www.omg.org/spec/EDMC-SR/FND/AgentsAndPeople/Agents/AutonomousAgent"/>
   </owl:ObjectProperty>

   <owl:ObjectProperty rdf:about="http://www.omg.org/spec/EDMC-SR/FND/Organizations/Organizations/organizationHasPart">
      <skos:definition>Some part of the organization, which is itself an organization.</skos:definition>
      <rdfs:subPropertyOf rdf:resource="http://www.omg.org/spec/EDMC-SR/FND/Relations/Relations/hasPart"/>
      <rdfs:domain rdf:resource="http://www.omg.org/spec/EDMC-SR/FND/Organizations/Organizations/Organization"/>
      <rdfs:range rdf:resource="http://www.omg.org/spec/EDMC-SR/FND/Organizations/Organizations/Organization"/>
   </owl:ObjectProperty>

   <owl:ObjectProperty rdf:about="http://www.omg.org/spec/EDMC-SR/FND/Organizations/Organizations/organizationHasAddress">
      <skos:definition>The address at which the organization is known and may receive correspondence.</skos:definition>
      <rdfs:subPropertyOf rdf:resource="http://www.edmcouncil.org/spec/EDMC-SR/FND/Information/InfoCore/details"/>
      <rdfs:domain rdf:resource="http://www.omg.org/spec/EDMC-SR/FND/Organizations/Organizations/Organization"/>
      <rdfs:range rdf:resource="http://www.omg.org/spec/EDMC-SR/FND/Places/Addresses/PostalAddress"/>
   </owl:ObjectProperty>

   <!--Data Properties-->

<!--Annotation Properties-->

<!--Classes-->

<owl:Class rdf:about="http://www.omg.org/spec/EDMC-SR/FND/Organizations/Organizations/Organization">
      <rdfs:label>Organization</rdfs:label>
      <rdfs:subClassOf rdf:resource="http://www.omg.org/spec/EDMC-SR/FND/AgentsAndPeople/Agents/AutonomousAgent"/>
   </owl:Class>

   <!--Individuals-->

</rdf:RDF>