<?xml version="1.0" encoding="UTF-8"?>
<!DOCTYPE rdf:RDF [
	<!ENTITY dct "http://purl.org/dc/terms/">
	<!ENTITY fibo-be-le-cb "https://spec.edmcouncil.org/fibo/ontology/BE/LegalEntities/CorporateBodies/">
	<!ENTITY fibo-be-le-fbo "https://spec.edmcouncil.org/fibo/ontology/BE/LegalEntities/FormalBusinessOrganizations/">
	<!ENTITY fibo-be-le-lp "https://spec.edmcouncil.org/fibo/ontology/BE/LegalEntities/LegalPersons/">
	<!ENTITY fibo-be-oac-cpty "https://spec.edmcouncil.org/fibo/ontology/BE/OwnershipAndControl/ControlParties/">
	<!ENTITY fibo-be-oac-opty "https://spec.edmcouncil.org/fibo/ontology/BE/OwnershipAndControl/OwnershipParties/">
	<!ENTITY fibo-be-ptr-ptr "https://spec.edmcouncil.org/fibo/ontology/BE/Partnerships/Partnerships/">
	<!ENTITY fibo-fnd-acc-aeq "https://spec.edmcouncil.org/fibo/ontology/FND/Accounting/AccountingEquity/">
	<!ENTITY fibo-fnd-agr-ctr "https://spec.edmcouncil.org/fibo/ontology/FND/Agreements/Contracts/">
	<!ENTITY fibo-fnd-law-lcap "https://spec.edmcouncil.org/fibo/ontology/FND/Law/LegalCapacity/">
	<!ENTITY fibo-fnd-oac-own "https://spec.edmcouncil.org/fibo/ontology/FND/OwnershipAndControl/Ownership/">
	<!ENTITY fibo-fnd-pty-pty "https://spec.edmcouncil.org/fibo/ontology/FND/Parties/Parties/">
	<!ENTITY fibo-fnd-pty-rl "https://spec.edmcouncil.org/fibo/ontology/FND/Parties/Roles/">
	<!ENTITY fibo-fnd-rel-rel "https://spec.edmcouncil.org/fibo/ontology/FND/Relations/Relations/">
	<!ENTITY fibo-fnd-utl-av "https://spec.edmcouncil.org/fibo/ontology/FND/Utilities/AnnotationVocabulary/">
	<!ENTITY owl "http://www.w3.org/2002/07/owl#">
	<!ENTITY rdf "http://www.w3.org/1999/02/22-rdf-syntax-ns#">
	<!ENTITY rdfs "http://www.w3.org/2000/01/rdf-schema#">
	<!ENTITY skos "http://www.w3.org/2004/02/skos/core#">
	<!ENTITY sm "http://www.omg.org/techprocess/ab/SpecificationMetadata/">
	<!ENTITY xsd "http://www.w3.org/2001/XMLSchema#">
]>
<rdf:RDF xml:base="https://spec.edmcouncil.org/fibo/ontology/BE/Partnerships/Partnerships/"
	xmlns:dct="http://purl.org/dc/terms/"
	xmlns:fibo-be-le-cb="https://spec.edmcouncil.org/fibo/ontology/BE/LegalEntities/CorporateBodies/"
	xmlns:fibo-be-le-fbo="https://spec.edmcouncil.org/fibo/ontology/BE/LegalEntities/FormalBusinessOrganizations/"
	xmlns:fibo-be-le-lp="https://spec.edmcouncil.org/fibo/ontology/BE/LegalEntities/LegalPersons/"
	xmlns:fibo-be-oac-cpty="https://spec.edmcouncil.org/fibo/ontology/BE/OwnershipAndControl/ControlParties/"
	xmlns:fibo-be-oac-opty="https://spec.edmcouncil.org/fibo/ontology/BE/OwnershipAndControl/OwnershipParties/"
	xmlns:fibo-be-ptr-ptr="https://spec.edmcouncil.org/fibo/ontology/BE/Partnerships/Partnerships/"
	xmlns:fibo-fnd-acc-aeq="https://spec.edmcouncil.org/fibo/ontology/FND/Accounting/AccountingEquity/"
	xmlns:fibo-fnd-agr-ctr="https://spec.edmcouncil.org/fibo/ontology/FND/Agreements/Contracts/"
	xmlns:fibo-fnd-law-lcap="https://spec.edmcouncil.org/fibo/ontology/FND/Law/LegalCapacity/"
	xmlns:fibo-fnd-oac-own="https://spec.edmcouncil.org/fibo/ontology/FND/OwnershipAndControl/Ownership/"
	xmlns:fibo-fnd-pty-pty="https://spec.edmcouncil.org/fibo/ontology/FND/Parties/Parties/"
	xmlns:fibo-fnd-pty-rl="https://spec.edmcouncil.org/fibo/ontology/FND/Parties/Roles/"
	xmlns:fibo-fnd-rel-rel="https://spec.edmcouncil.org/fibo/ontology/FND/Relations/Relations/"
	xmlns:fibo-fnd-utl-av="https://spec.edmcouncil.org/fibo/ontology/FND/Utilities/AnnotationVocabulary/"
	xmlns:owl="http://www.w3.org/2002/07/owl#"
	xmlns:rdf="http://www.w3.org/1999/02/22-rdf-syntax-ns#"
	xmlns:rdfs="http://www.w3.org/2000/01/rdf-schema#"
	xmlns:skos="http://www.w3.org/2004/02/skos/core#"
	xmlns:sm="http://www.omg.org/techprocess/ab/SpecificationMetadata/"
	xmlns:xsd="http://www.w3.org/2001/XMLSchema#">
	
	<owl:Ontology rdf:about="https://spec.edmcouncil.org/fibo/ontology/BE/Partnerships/Partnerships/">
		<rdfs:label>Partnerships Ontology</rdfs:label>
		<dct:abstract>This ontology defines partnerships and related concepts. The concepts distinguish general from limited partners, as well as the types of equity that they hold. Included are abstract definitions of partnership types based on whether they have general, limited or both kinds of partners. Both legally incorporated and non incorporated forms of partnerships are covered.</dct:abstract>
		<dct:license rdf:datatype="&xsd;anyURI">http://opensource.org/licenses/MIT</dct:license>
		<sm:contentLanguage rdf:datatype="&xsd;anyURI">http://www.w3.org/standards/techs/owl#w3c_all</sm:contentLanguage>
		<sm:copyright>Copyright (c) 2013-2018 EDM Council, Inc.</sm:copyright>
		<sm:copyright>Copyright (c) 2013-2018 Object Management Group, Inc.</sm:copyright>
		<sm:dependsOn rdf:datatype="&xsd;anyURI">https://spec.edmcouncil.org/fibo/ontology/BE/LegalEntities/CorporateBodies/</sm:dependsOn>
		<sm:dependsOn rdf:datatype="&xsd;anyURI">https://spec.edmcouncil.org/fibo/ontology/BE/LegalEntities/FormalBusinessOrganizations/</sm:dependsOn>
		<sm:dependsOn rdf:datatype="&xsd;anyURI">https://spec.edmcouncil.org/fibo/ontology/BE/LegalEntities/LegalPersons/</sm:dependsOn>
		<sm:dependsOn rdf:datatype="&xsd;anyURI">https://spec.edmcouncil.org/fibo/ontology/BE/OwnershipAndControl/ControlParties/</sm:dependsOn>
		<sm:dependsOn rdf:datatype="&xsd;anyURI">https://spec.edmcouncil.org/fibo/ontology/BE/OwnershipAndControl/OwnershipParties/</sm:dependsOn>
		<sm:dependsOn rdf:datatype="&xsd;anyURI">https://spec.edmcouncil.org/fibo/ontology/FND/</sm:dependsOn>
		<sm:fileAbbreviation>fibo-be-ptr-ptr</sm:fileAbbreviation>
		<sm:filename>Partnerships.rdf</sm:filename>
		<owl:imports rdf:resource="https://spec.edmcouncil.org/fibo/ontology/BE/LegalEntities/CorporateBodies/"/>
		<owl:imports rdf:resource="https://spec.edmcouncil.org/fibo/ontology/BE/LegalEntities/FormalBusinessOrganizations/"/>
		<owl:imports rdf:resource="https://spec.edmcouncil.org/fibo/ontology/BE/LegalEntities/LegalPersons/"/>
		<owl:imports rdf:resource="https://spec.edmcouncil.org/fibo/ontology/BE/OwnershipAndControl/ControlParties/"/>
		<owl:imports rdf:resource="https://spec.edmcouncil.org/fibo/ontology/BE/OwnershipAndControl/OwnershipParties/"/>
		<owl:imports rdf:resource="https://spec.edmcouncil.org/fibo/ontology/FND/Accounting/AccountingEquity/"/>
		<owl:imports rdf:resource="https://spec.edmcouncil.org/fibo/ontology/FND/Agreements/Contracts/"/>
		<owl:imports rdf:resource="https://spec.edmcouncil.org/fibo/ontology/FND/Law/LegalCapacity/"/>
		<owl:imports rdf:resource="https://spec.edmcouncil.org/fibo/ontology/FND/OwnershipAndControl/Ownership/"/>
		<owl:imports rdf:resource="https://spec.edmcouncil.org/fibo/ontology/FND/Parties/Parties/"/>
		<owl:imports rdf:resource="https://spec.edmcouncil.org/fibo/ontology/FND/Parties/Roles/"/>
		<owl:imports rdf:resource="https://spec.edmcouncil.org/fibo/ontology/FND/Relations/Relations/"/>
		<owl:imports rdf:resource="https://spec.edmcouncil.org/fibo/ontology/FND/Utilities/AnnotationVocabulary/"/>
		<owl:versionIRI rdf:resource="https://spec.edmcouncil.org/fibo/ontology/BE/20181101/Partnerships/Partnerships/"/>
		<skos:changeNote>The https://spec.edmcouncil.org/fibo/ontology/BE/20131101/Partnerships/Partnerships.rdf version of this ontology was modified per the issue resolutions identified in the FIBO BE 1.0 FTF report.</skos:changeNote>
		<skos:changeNote>The https://spec.edmcouncil.org/fibo/ontology/BE/20160201/Partnerships/Partnerships.rdf version of this ontology was modified per the FIBO 2.0 RFC to reference shareholders&apos; equity vs. stockholders&apos; equity and correct a number of restrictions.</skos:changeNote>
		<skos:changeNote>The https://spec.edmcouncil.org/fibo/ontology/BE/20180801/Partnerships/Partnerships.rdf version of this ontology was modified to simplify / merge the legal person and formal organization class hierarchies.</skos:changeNote>
		<fibo-fnd-utl-av:hasMaturityLevel rdf:resource="&fibo-fnd-utl-av;Release"/>
	</owl:Ontology>
	
	<owl:Class rdf:about="&fibo-be-ptr-ptr;CorporateLimitedPartner">
		<rdfs:subClassOf rdf:resource="&fibo-be-ptr-ptr;LimitedPartner"/>
		<rdfs:subClassOf>
			<owl:Restriction>
				<owl:onProperty rdf:resource="&fibo-fnd-rel-rel;hasIdentity"/>
				<owl:onClass rdf:resource="&fibo-be-le-cb;Corporation"/>
				<owl:qualifiedCardinality rdf:datatype="&xsd;nonNegativeInteger">1</owl:qualifiedCardinality>
			</owl:Restriction>
		</rdfs:subClassOf>
		<rdfs:label>corporate limited partner</rdfs:label>
		<skos:definition>A limited partner in a partnership, who is and may only be a Corporate Legal Person (i.e., not a natural person)</skos:definition>
	</owl:Class>
	
	<owl:Class rdf:about="&fibo-be-ptr-ptr;EquityApportionmentTermsSet">
		<rdfs:subClassOf rdf:resource="&fibo-fnd-agr-ctr;ContractualCommitment"/>
		<rdfs:label>equity apportionment terms set</rdfs:label>
		<skos:definition>contract terms defining the apportionment of equity for some formal business organization.</skos:definition>
	</owl:Class>
	
	<owl:Class rdf:about="&fibo-be-ptr-ptr;GeneralPartner">
		<rdfs:subClassOf rdf:resource="&fibo-be-oac-cpty;DeJureControllingInterestParty"/>
		<rdfs:subClassOf rdf:resource="&fibo-be-ptr-ptr;Partner"/>
		<rdfs:subClassOf>
			<owl:Restriction>
				<owl:onProperty rdf:resource="&fibo-fnd-rel-rel;hasIdentity"/>
				<owl:onClass rdf:resource="&fibo-be-le-lp;LegallyCompetentNaturalPerson"/>
				<owl:qualifiedCardinality rdf:datatype="&xsd;nonNegativeInteger">1</owl:qualifiedCardinality>
			</owl:Restriction>
		</rdfs:subClassOf>
		<rdfs:subClassOf>
			<owl:Restriction>
				<owl:onProperty rdf:resource="&fibo-be-oac-opty;holdsEquityIn"/>
				<owl:someValuesFrom rdf:resource="&fibo-be-ptr-ptr;GeneralPartnerEquity"/>
			</owl:Restriction>
		</rdfs:subClassOf>
		<rdfs:subClassOf>
			<owl:Restriction>
				<owl:onProperty rdf:resource="&fibo-fnd-pty-rl;isPlayedBy"/>
				<owl:someValuesFrom>
					<owl:Restriction>
						<owl:onProperty rdf:resource="&fibo-fnd-law-lcap;hasCapacity"/>
						<owl:allValuesFrom rdf:resource="&fibo-fnd-law-lcap;LiabilityCapacity"/>
					</owl:Restriction>
				</owl:someValuesFrom>
			</owl:Restriction>
		</rdfs:subClassOf>
		<rdfs:label>general partner</rdfs:label>
		<skos:definition>a partner in a partnership, who holds some part of the general partner equity and typically is jointly and severally liable with the other partners for the liabilities incurred by that partnership</skos:definition>
	</owl:Class>
	
	<owl:Class rdf:about="&fibo-be-ptr-ptr;GeneralPartnerEquity">
		<rdfs:subClassOf rdf:resource="&fibo-be-oac-opty;ControllingEquity"/>
		<rdfs:subClassOf rdf:resource="&fibo-be-ptr-ptr;PartnershipEquity"/>
		<rdfs:subClassOf>
			<owl:Restriction>
				<owl:onProperty rdf:resource="&fibo-fnd-rel-rel;confers"/>
				<owl:allValuesFrom rdf:resource="&fibo-be-oac-cpty;ConstitutionalDeJureControl"/>
			</owl:Restriction>
		</rdfs:subClassOf>
		<rdfs:label>general partner equity</rdfs:label>
		<skos:definition>Equity in a partnership held by general partners; this is typically accompanied by full liability capability on the part of the holders of the equity.</skos:definition>
		<skos:editorialNote>For a typical, non incorporated partnership, this is the only equity in the entity. Other typically incorporated partnerships may have additional limited equity in addition to or instead of this.</skos:editorialNote>
	</owl:Class>
	
	<owl:Class rdf:about="&fibo-be-ptr-ptr;LegallyIncorporatedPartnership">
		<rdfs:subClassOf rdf:resource="&fibo-be-ptr-ptr;Partnership"/>
		<rdfs:subClassOf>
			<owl:Restriction>
				<owl:onProperty rdf:resource="&fibo-fnd-rel-rel;hasMember"/>
				<owl:onClass>
					<owl:Restriction>
						<owl:onProperty rdf:resource="&fibo-fnd-pty-rl;playsRole"/>
						<owl:someValuesFrom rdf:resource="&fibo-be-ptr-ptr;LegallyIncorporatedPartnershipMember"/>
					</owl:Restriction>
				</owl:onClass>
				<owl:minQualifiedCardinality rdf:datatype="&xsd;nonNegativeInteger">2</owl:minQualifiedCardinality>
			</owl:Restriction>
		</rdfs:subClassOf>
		<rdfs:label>legally incorporated partnership</rdfs:label>
		<owl:deprecated rdf:datatype="&xsd;boolean">true</owl:deprecated>
		<skos:definition>Any partnership which is defined as a legal person within a given jurisdiction, for example a limited liability partnership (if that is a legal person).</skos:definition>
		<skos:editorialNote>The precise details and definition of these may vary from one jurisdiction to another. This type of entity is defined by being a legal person in its own right, as distinct from the usual type of partnership where the partners remain jointly and severally liable for debts.</skos:editorialNote>
	</owl:Class>
	
	<owl:Class rdf:about="&fibo-be-ptr-ptr;LegallyIncorporatedPartnershipMember">
		<rdfs:subClassOf rdf:resource="&fibo-be-ptr-ptr;Partner"/>
		<rdfs:label>legally incorporated partnership member</rdfs:label>
		<owl:deprecated rdf:datatype="&xsd;boolean">true</owl:deprecated>
		<skos:definition>a party that is a member or partner in a legally incorporated partnership such as an LLC or LLP</skos:definition>
	</owl:Class>
	
	<owl:Class rdf:about="&fibo-be-ptr-ptr;LiabilityApportionmentTermsSet">
		<rdfs:subClassOf rdf:resource="&fibo-fnd-agr-ctr;ContractualCommitment"/>
		<rdfs:label>liability apportionment terms set</rdfs:label>
		<skos:definition>terms defining the apportionment of liabilities accrued by some formal business organization.</skos:definition>
	</owl:Class>
	
	<owl:Class rdf:about="&fibo-be-ptr-ptr;LimitedPartner">
		<rdfs:subClassOf rdf:resource="&fibo-be-ptr-ptr;Partner"/>
		<rdfs:subClassOf>
			<owl:Restriction>
				<owl:onProperty rdf:resource="&fibo-be-oac-opty;holdsEquityIn"/>
				<owl:someValuesFrom rdf:resource="&fibo-be-ptr-ptr;LimitedPartnerEquity"/>
			</owl:Restriction>
		</rdfs:subClassOf>
		<rdfs:label>limited partner</rdfs:label>
		<skos:definition>a partner whose liabilities are limited to the extent of their equity holding or guarantees</skos:definition>
	</owl:Class>
	
	<owl:Class rdf:about="&fibo-be-ptr-ptr;LimitedPartnerEquity">
		<rdfs:subClassOf rdf:resource="&fibo-be-ptr-ptr;PartnershipEquity"/>
		<rdfs:label>limited partner equity</rdfs:label>
		<skos:definition>equity in a partnership held by limited partners; this is not accompanied by any liability capability on the part of the holders of this equity.</skos:definition>
	</owl:Class>
	
	<owl:Class rdf:about="&fibo-be-ptr-ptr;NaturalPersonLimitedPartner">
		<rdfs:subClassOf rdf:resource="&fibo-be-ptr-ptr;LimitedPartner"/>
		<rdfs:subClassOf>
			<owl:Restriction>
				<owl:onProperty rdf:resource="&fibo-fnd-rel-rel;hasIdentity"/>
				<owl:onClass rdf:resource="&fibo-be-le-lp;LegallyCompetentNaturalPerson"/>
				<owl:qualifiedCardinality rdf:datatype="&xsd;nonNegativeInteger">1</owl:qualifiedCardinality>
			</owl:Restriction>
		</rdfs:subClassOf>
		<rdfs:label>natural person limited partner</rdfs:label>
		<skos:definition>a limited partner in a partnership who is a natural person</skos:definition>
	</owl:Class>
	
	<owl:Class rdf:about="&fibo-be-ptr-ptr;NonIncorporatedPartnership">
		<rdfs:subClassOf rdf:resource="&fibo-be-ptr-ptr;PartnershipWithGeneralPartners"/>
		<rdfs:label>non-incorporated partnership</rdfs:label>
		<skos:definition>a partnership in which the partners are jointly and severally liable for liabilities incurred by the entity</skos:definition>
	</owl:Class>
	
	<owl:Class rdf:about="&fibo-be-ptr-ptr;Partner">
		<rdfs:subClassOf rdf:resource="&fibo-be-le-fbo;FormallyConstitutedOrganizationMember"/>
		<rdfs:subClassOf rdf:resource="&fibo-be-oac-opty;ConstitutionalOwner"/>
		<rdfs:subClassOf>
			<owl:Restriction>
				<owl:onProperty rdf:resource="&fibo-fnd-rel-rel;hasIdentity"/>
				<owl:onClass rdf:resource="&fibo-be-le-lp;LegalPerson"/>
				<owl:qualifiedCardinality rdf:datatype="&xsd;nonNegativeInteger">1</owl:qualifiedCardinality>
			</owl:Restriction>
		</rdfs:subClassOf>
		<rdfs:subClassOf>
			<owl:Restriction>
				<owl:onProperty rdf:resource="&fibo-fnd-pty-rl;isPlayedBy"/>
				<owl:someValuesFrom>
					<owl:Restriction>
						<owl:onProperty rdf:resource="&fibo-fnd-rel-rel;isMemberOf"/>
						<owl:allValuesFrom rdf:resource="&fibo-be-ptr-ptr;Partnership"/>
					</owl:Restriction>
				</owl:someValuesFrom>
			</owl:Restriction>
		</rdfs:subClassOf>
		<rdfs:subClassOf>
			<owl:Restriction>
				<owl:onProperty rdf:resource="&fibo-fnd-pty-rl;isPlayedBy"/>
				<owl:someValuesFrom>
					<owl:Restriction>
						<owl:onProperty rdf:resource="&fibo-fnd-pty-pty;isAPartyTo"/>
						<owl:onClass rdf:resource="&fibo-be-ptr-ptr;PartnershipAgreement"/>
						<owl:qualifiedCardinality rdf:datatype="&xsd;nonNegativeInteger">1</owl:qualifiedCardinality>
					</owl:Restriction>
				</owl:someValuesFrom>
			</owl:Restriction>
		</rdfs:subClassOf>
		<rdfs:label>partner</rdfs:label>
		<skos:definition>a member of a partnership</skos:definition>
		<skos:scopeNote>This term is not referred to directly in specific kinds of partnership. Nearly all partnerships have General Partners, while forms of (mostly legally incorporated) partnerships have in addition Limited Partners. This term is the common ancestor of both.</skos:scopeNote>
		<fibo-fnd-utl-av:definitionOrigin rdf:datatype="&xsd;anyURI">http://www.investorwords.com/3608/partner.html</fibo-fnd-utl-av:definitionOrigin>
	</owl:Class>
	
	<owl:Class rdf:about="&fibo-be-ptr-ptr;Partnership">
		<rdfs:subClassOf rdf:resource="&fibo-be-le-fbo;FormallyConstitutedOrganization"/>
		<rdfs:subClassOf rdf:resource="&fibo-be-le-lp;LegalEntity"/>
		<rdfs:subClassOf>
			<owl:Restriction>
				<owl:onProperty rdf:resource="&fibo-be-le-lp;hasObjective"/>
				<owl:onClass rdf:resource="&fibo-be-le-lp;ProfitObjective"/>
				<owl:minQualifiedCardinality rdf:datatype="&xsd;nonNegativeInteger">0</owl:minQualifiedCardinality>
			</owl:Restriction>
		</rdfs:subClassOf>
		<rdfs:subClassOf>
			<owl:Restriction>
				<owl:onProperty rdf:resource="&fibo-fnd-rel-rel;hasMember"/>
				<owl:onClass>
					<owl:Restriction>
						<owl:onProperty rdf:resource="&fibo-fnd-pty-rl;playsRole"/>
						<owl:someValuesFrom rdf:resource="&fibo-be-ptr-ptr;Partner"/>
					</owl:Restriction>
				</owl:onClass>
				<owl:minQualifiedCardinality rdf:datatype="&xsd;nonNegativeInteger">2</owl:minQualifiedCardinality>
			</owl:Restriction>
		</rdfs:subClassOf>
		<rdfs:subClassOf>
			<owl:Restriction>
				<owl:onProperty rdf:resource="&fibo-be-le-fbo;hasEquity"/>
				<owl:someValuesFrom rdf:resource="&fibo-be-ptr-ptr;PartnershipEquity"/>
			</owl:Restriction>
		</rdfs:subClassOf>
		<rdfs:subClassOf>
			<owl:Restriction>
				<owl:onProperty rdf:resource="&fibo-fnd-rel-rel;isGovernedBy"/>
				<owl:someValuesFrom rdf:resource="&fibo-be-ptr-ptr;PartnershipAgreement"/>
			</owl:Restriction>
		</rdfs:subClassOf>
		<rdfs:label>partnership</rdfs:label>
		<skos:definition>venture in which two or more legal entities carry out some business activities under a common identity</skos:definition>
		<skos:editorialNote>If the partnership doesn&apos;t limit the liability of the partners then the party to the contract is a natural person. If it does, then it&apos;s an artificial legal person (Body Corporate) - see Legally Incorporated Partnerships. Scope Note: This term of Partnership in the most general sense is ancestral to both of those.</skos:editorialNote>
	</owl:Class>
	
	<owl:Class rdf:about="&fibo-be-ptr-ptr;PartnershipAgreement">
		<rdfs:subClassOf rdf:resource="&fibo-be-le-fbo;OrganizationCoveringAgreement"/>
		<rdfs:subClassOf>
			<owl:Restriction>
				<owl:onProperty rdf:resource="&fibo-fnd-agr-ctr;hasContractualElement"/>
				<owl:someValuesFrom rdf:resource="&fibo-be-ptr-ptr;EquityApportionmentTermsSet"/>
			</owl:Restriction>
		</rdfs:subClassOf>
		<rdfs:subClassOf>
			<owl:Restriction>
				<owl:onProperty rdf:resource="&fibo-fnd-agr-ctr;hasContractualElement"/>
				<owl:someValuesFrom rdf:resource="&fibo-be-ptr-ptr;LiabilityApportionmentTermsSet"/>
			</owl:Restriction>
		</rdfs:subClassOf>
		<rdfs:subClassOf>
			<owl:Restriction>
				<owl:onProperty rdf:resource="&fibo-fnd-pty-pty;hasPartyInRole"/>
				<owl:someValuesFrom rdf:resource="&fibo-be-ptr-ptr;Partner"/>
			</owl:Restriction>
		</rdfs:subClassOf>
		<rdfs:label>partnership agreement</rdfs:label>
		<skos:definition>a document setting up a partnership, giving the details of the business and the amount each partner is contributing to it.</skos:definition>
		<fibo-fnd-utl-av:synonym>articles of partnership</fibo-fnd-utl-av:synonym>
	</owl:Class>
	
	<owl:Class rdf:about="&fibo-be-ptr-ptr;PartnershipEquity">
		<rdfs:subClassOf rdf:resource="&fibo-fnd-acc-aeq;OwnersEquity"/>
		<rdfs:subClassOf>
			<owl:Restriction>
				<owl:onProperty rdf:resource="&fibo-fnd-acc-aeq;representsAnInterestIn"/>
				<owl:someValuesFrom rdf:resource="&fibo-be-ptr-ptr;Partnership"/>
			</owl:Restriction>
		</rdfs:subClassOf>
		<rdfs:label>partnership equity</rdfs:label>
		<skos:definition>equity in some partnership</skos:definition>
	</owl:Class>
	
	<owl:Class rdf:about="&fibo-be-ptr-ptr;PartnershipIncorporatedByEquity">
		<rdfs:subClassOf rdf:resource="&fibo-be-ptr-ptr;PartnershipWithLimitedPartners"/>
		<rdfs:label>partnership incorporated by equity</rdfs:label>
		<skos:definition>a partnership incorporated via the issuance of equity, with limited partners (i.e., partners whose liability is limited) that are necessarily not natural persons (i.e., cannot be individuals)</skos:definition>
	</owl:Class>
	
	<owl:Class rdf:about="&fibo-be-ptr-ptr;PartnershipIncorporatedThroughAgreement">
		<rdfs:subClassOf rdf:resource="&fibo-be-le-cb;BodyIncorporatedThroughAgreement"/>
		<rdfs:subClassOf rdf:resource="&fibo-be-ptr-ptr;Partnership"/>
		<rdfs:label>partnership incorporated through agreement</rdfs:label>
		<skos:definition>a partnership which has legal personhood, but for which there is not some issuance of limited partner equity</skos:definition>
		<skos:editorialNote>An LLP (in the UK) is an example of this - in this case, the LLP document is the legal document which effectively constitutes the partnership</skos:editorialNote>
	</owl:Class>
	
	<owl:Class rdf:about="&fibo-be-ptr-ptr;PartnershipWithCorporateLimitedPartners">
		<rdfs:subClassOf rdf:resource="&fibo-be-ptr-ptr;PartnershipWithLimitedPartners"/>
		<rdfs:subClassOf>
			<owl:Restriction>
				<owl:onProperty rdf:resource="&fibo-fnd-rel-rel;hasMember"/>
				<owl:someValuesFrom>
					<owl:Restriction>
						<owl:onProperty rdf:resource="&fibo-fnd-pty-rl;playsRole"/>
						<owl:someValuesFrom rdf:resource="&fibo-be-ptr-ptr;CorporateLimitedPartner"/>
					</owl:Restriction>
				</owl:someValuesFrom>
			</owl:Restriction>
		</rdfs:subClassOf>
		<rdfs:label>partnership with corporate limited partners</rdfs:label>
		<owl:disjointWith rdf:resource="&fibo-be-ptr-ptr;PartnershipWithNaturalPersonLimitedPartners"/>
		<skos:definition>A partnership with limited partners (partners whose liability is limited) and where those partners are necessarily non natural persons (i.e. cannot be individuals).</skos:definition>
	</owl:Class>
	
	<owl:Class rdf:about="&fibo-be-ptr-ptr;PartnershipWithGeneralAndLimitedPartners">
		<rdfs:subClassOf rdf:resource="&fibo-be-ptr-ptr;PartnershipWithGeneralPartners"/>
		<rdfs:subClassOf rdf:resource="&fibo-be-ptr-ptr;PartnershipWithLimitedPartners"/>
		<rdfs:label>partnership with general and limited partners</rdfs:label>
		<owl:disjointWith rdf:resource="&fibo-be-ptr-ptr;PartnershipWithOnlyLimitedPartners"/>
		<skos:definition>a partnership having both limited partners and general partners</skos:definition>
	</owl:Class>
	
	<owl:Class rdf:about="&fibo-be-ptr-ptr;PartnershipWithGeneralPartners">
		<rdfs:subClassOf rdf:resource="&fibo-be-ptr-ptr;Partnership"/>
		<rdfs:subClassOf>
			<owl:Restriction>
				<owl:onProperty rdf:resource="&fibo-fnd-rel-rel;hasMember"/>
				<owl:onClass>
					<owl:Restriction>
						<owl:onProperty rdf:resource="&fibo-fnd-pty-rl;playsRole"/>
						<owl:someValuesFrom rdf:resource="&fibo-be-ptr-ptr;GeneralPartner"/>
					</owl:Restriction>
				</owl:onClass>
				<owl:minQualifiedCardinality rdf:datatype="&xsd;nonNegativeInteger">2</owl:minQualifiedCardinality>
			</owl:Restriction>
		</rdfs:subClassOf>
		<rdfs:label>partnership with general partners</rdfs:label>
		<skos:definition>a partnership that has two or more general partners</skos:definition>
		<skos:editorialNote>The partnership may or may not also have limited partners. In a typical non-incorporated partnership, it does not. General partners of a partnership must be natural persons.</skos:editorialNote>
	</owl:Class>
	
	<owl:Class rdf:about="&fibo-be-ptr-ptr;PartnershipWithGeneralPartnersWithLimitedLiability">
		<rdfs:subClassOf rdf:resource="&fibo-be-ptr-ptr;PartnershipWithGeneralPartners"/>
		<rdfs:label>partnership with general partners with limited liability</rdfs:label>
		<skos:definition>a partnership that has general partners, whose general partners have limited liability</skos:definition>
		<skos:scopeNote>This is therefore necessarily a legal person (no-one else has liability); example in some US states is a limited liability limited partnership.</skos:scopeNote>
	</owl:Class>
	
	<owl:Class rdf:about="&fibo-be-ptr-ptr;PartnershipWithLimitedPartners">
		<rdfs:subClassOf rdf:resource="&fibo-be-ptr-ptr;Partnership"/>
		<rdfs:subClassOf>
			<owl:Restriction>
				<owl:onProperty rdf:resource="&fibo-fnd-rel-rel;hasMember"/>
				<owl:someValuesFrom>
					<owl:Restriction>
						<owl:onProperty rdf:resource="&fibo-fnd-pty-rl;playsRole"/>
						<owl:someValuesFrom rdf:resource="&fibo-be-ptr-ptr;LimitedPartner"/>
					</owl:Restriction>
				</owl:someValuesFrom>
			</owl:Restriction>
		</rdfs:subClassOf>
		<rdfs:label>partnership with limited partners</rdfs:label>
		<skos:definition>a partnership having limited partners, that is partners whose liabilities are limited to the extent of their equity or guarantees</skos:definition>
		<skos:editorialNote>Possibly but not necessarily a Legal Person. If there are only Limited Partners then this is of necessity a Legal Person (no-one else has liability in this structure).</skos:editorialNote>
	</owl:Class>
	
	<owl:Class rdf:about="&fibo-be-ptr-ptr;PartnershipWithNaturalPersonLimitedPartners">
		<rdfs:subClassOf rdf:resource="&fibo-be-ptr-ptr;PartnershipWithLimitedPartners"/>
		<rdfs:subClassOf>
			<owl:Restriction>
				<owl:onProperty rdf:resource="&fibo-fnd-rel-rel;hasMember"/>
				<owl:someValuesFrom>
					<owl:Restriction>
						<owl:onProperty rdf:resource="&fibo-fnd-pty-rl;playsRole"/>
						<owl:someValuesFrom rdf:resource="&fibo-be-ptr-ptr;NaturalPersonLimitedPartner"/>
					</owl:Restriction>
				</owl:someValuesFrom>
			</owl:Restriction>
		</rdfs:subClassOf>
		<rdfs:label>partnership with natural person limited partners</rdfs:label>
		<skos:definition>a partnership with limited partners (partners whose liability is limited) and where those partners are necessarily natural persons (i.e. cannot be corporates)</skos:definition>
		<skos:scopeNote>Example in US, a Limited Liability Partnership</skos:scopeNote>
	</owl:Class>
	
	<owl:Class rdf:about="&fibo-be-ptr-ptr;PartnershipWithOnlyLimitedPartners">
		<rdfs:subClassOf rdf:resource="&fibo-be-ptr-ptr;PartnershipWithLimitedPartners"/>
		<rdfs:label>partnership with only limited partners</rdfs:label>
		<skos:definition>a partnership having limited partners but no general partners</skos:definition>
	</owl:Class>
	
	<owl:DatatypeProperty rdf:about="&fibo-be-ptr-ptr;dateTradingFrom">
		<rdfs:label>date trading from</rdfs:label>
		<rdfs:range rdf:resource="&xsd;dateTime"/>
		<skos:definition>date on which the partnership started trading</skos:definition>
	</owl:DatatypeProperty>
	
	<owl:ObjectProperty rdf:about="&fibo-be-ptr-ptr;holdsPartnershipEquityIn">
		<rdfs:subPropertyOf rdf:resource="&fibo-fnd-oac-own;owns"/>
		<rdfs:label>holds partnership equity in</rdfs:label>
		<rdfs:range rdf:resource="&fibo-be-ptr-ptr;PartnershipEquity"/>
		<owl:deprecated rdf:datatype="&xsd;boolean">true</owl:deprecated>
		<skos:definition>relates a partner to the equity that partner holds in the partnership</skos:definition>
	</owl:ObjectProperty>
	
	<owl:ObjectProperty rdf:about="&fibo-be-ptr-ptr;setsOutEquityTermsIn">
		<rdfs:subPropertyOf rdf:resource="&fibo-fnd-agr-ctr;hasTerms"/>
		<rdfs:label>sets out equity terms in</rdfs:label>
		<rdfs:domain rdf:resource="&fibo-be-le-fbo;OrganizationCoveringAgreement"/>
		<rdfs:range rdf:resource="&fibo-be-ptr-ptr;EquityApportionmentTermsSet"/>
		<owl:deprecated rdf:datatype="&xsd;boolean">true</owl:deprecated>
		<skos:definition>has terms setting out the apportionment of equity in some formal business organization</skos:definition>
	</owl:ObjectProperty>
	
	<owl:ObjectProperty rdf:about="&fibo-be-ptr-ptr;setsOutLiabilityTermsIn">
		<rdfs:subPropertyOf rdf:resource="&fibo-fnd-agr-ctr;hasTerms"/>
		<rdfs:label>sets out liability terms in</rdfs:label>
		<rdfs:domain rdf:resource="&fibo-be-le-fbo;OrganizationCoveringAgreement"/>
		<rdfs:range rdf:resource="&fibo-be-ptr-ptr;LiabilityApportionmentTermsSet"/>
		<owl:deprecated rdf:datatype="&xsd;boolean">true</owl:deprecated>
		<skos:definition>has terms setting out the apportionment of liabilities for debts or other liabilities accrued by some formal business organization</skos:definition>
	</owl:ObjectProperty>

</rdf:RDF>