<?xml version="1.0" encoding="UTF-8"?>
<!DOCTYPE rdf:RDF [
	<!ENTITY fibo-fnd-math-math "https://spec.edmcouncil.org/fibo/FND/Math/Math/">
	<!ENTITY fibo-fnd-utl-av "https://spec.edmcouncil.org/fibo/FND/Utilities/AnnotationVocabulary/">
	<!ENTITY fibo-fnd-utlx-val "https://spec.edmcouncil.org/fibo/FND/UtilitiesExt/Values/">
	<!ENTITY fibo-md-dbtx-int "https://spec.edmcouncil.org/fibo/MD/DebtTemporal/DebtInterestAmounts/">
	<!ENTITY fibo-md-temx-ins "https://spec.edmcouncil.org/fibo/MD/TemporalCore/InstrumentTemporalTerms/">
	<!ENTITY fibo-md-temx-tem "https://spec.edmcouncil.org/fibo/MD/TemporalCore/TemporalConcepts/">
	<!ENTITY fibo-sec-dbt-bo-cft "https://spec.edmcouncil.org/fibo/SEC/Debt/Bonds/BondsCashflowTerms/">
	<!ENTITY owl "http://www.w3.org/2002/07/owl#">
	<!ENTITY rdf "http://www.w3.org/1999/02/22-rdf-syntax-ns#">
	<!ENTITY rdfs "http://www.w3.org/2000/01/rdf-schema#">
	<!ENTITY skos "http://www.w3.org/2004/02/skos/core#">
	<!ENTITY xsd "http://www.w3.org/2001/XMLSchema#">
]>
<rdf:RDF xml:base="https://spec.edmcouncil.org/fibo/MD/DebtTemporal/DebtInterestAmounts/"
	xmlns:fibo-fnd-math-math="https://spec.edmcouncil.org/fibo/FND/Math/Math/"
	xmlns:fibo-fnd-utl-av="https://spec.edmcouncil.org/fibo/FND/Utilities/AnnotationVocabulary/"
	xmlns:fibo-fnd-utlx-val="https://spec.edmcouncil.org/fibo/FND/UtilitiesExt/Values/"
	xmlns:fibo-md-dbtx-int="https://spec.edmcouncil.org/fibo/MD/DebtTemporal/DebtInterestAmounts/"
	xmlns:fibo-md-temx-ins="https://spec.edmcouncil.org/fibo/MD/TemporalCore/InstrumentTemporalTerms/"
	xmlns:fibo-md-temx-tem="https://spec.edmcouncil.org/fibo/MD/TemporalCore/TemporalConcepts/"
	xmlns:fibo-sec-dbt-bo-cft="https://spec.edmcouncil.org/fibo/SEC/Debt/Bonds/BondsCashflowTerms/"
	xmlns:owl="http://www.w3.org/2002/07/owl#"
	xmlns:rdf="http://www.w3.org/1999/02/22-rdf-syntax-ns#"
	xmlns:rdfs="http://www.w3.org/2000/01/rdf-schema#"
	xmlns:skos="http://www.w3.org/2004/02/skos/core#"
	xmlns:xsd="http://www.w3.org/2001/XMLSchema#">
	
	<owl:Ontology rdf:about="https://spec.edmcouncil.org/fibo/MD/DebtTemporal/DebtInterestAmounts/">
		<rdfs:label xml:lang="en">DebtInterestAmounts</rdfs:label>
		<owl:imports rdf:resource="http://www.w3.org/2004/02/skos/core"/>
		<owl:imports rdf:resource="https://spec.edmcouncil.org/fibo/FND/Math/Math/"/>
		<owl:imports rdf:resource="https://spec.edmcouncil.org/fibo/FND/Utilities/AnnotationVocabulary/"/>
		<owl:imports rdf:resource="https://spec.edmcouncil.org/fibo/FND/UtilitiesExt/Values/"/>
		<owl:imports rdf:resource="https://spec.edmcouncil.org/fibo/IND/Indicators/Indicators/"/>
		<owl:imports rdf:resource="https://spec.edmcouncil.org/fibo/MD/TemporalCore/InstrumentTemporalTerms/"/>
		<owl:imports rdf:resource="https://spec.edmcouncil.org/fibo/MD/TemporalCore/TemporalConcepts/"/>
		<owl:imports rdf:resource="https://spec.edmcouncil.org/fibo/SEC/Debt/Bonds/BondsCashflowTerms/"/>
		<owl:versionIRI rdf:resource="https://spec.edmcouncil.org/fibo/MD/DebtTemporal/DebtInterestAmounts/"/>
		<fibo-fnd-utl-av:hasMaturityLevel rdf:resource="&fibo-fnd-utl-av;Provisional"/>
	</owl:Ontology>
	
	<owl:Class rdf:about="&fibo-md-dbtx-int;BondCoupon">
		<rdfs:subClassOf rdf:resource="&fibo-fnd-math-math;ContractuallyDefinedNumericalParameter"/>
		<rdfs:subClassOf rdf:resource="&fibo-md-dbtx-int;DebtSecurityInterestAmount"/>
		<rdfs:label xml:lang="en">bond coupon</rdfs:label>
		<skos:definition xml:lang="en">Mechanism whereby an investor receives income from interest payments, which are usually made periodically.</skos:definition>
		<fibo-fnd-utl-av:synonym xml:lang="en">bond interest</fibo-fnd-utl-av:synonym>
	</owl:Class>
	
	<owl:Class rdf:about="&fibo-md-dbtx-int;BondFixedCoupon">
		<rdfs:subClassOf rdf:resource="&fibo-md-dbtx-int;BondCoupon"/>
		<rdfs:label xml:lang="en">bond fixed coupon</rdfs:label>
		<owl:disjointWith rdf:resource="&fibo-md-dbtx-int;BondVariableCoupon"/>
		<skos:definition xml:lang="en">Mechanism whereby an investor receives income from interest payments, which are usually made periodically. These are for a fixed amount.</skos:definition>
	</owl:Class>
	
	<owl:Class rdf:about="&fibo-md-dbtx-int;BondVariableCoupon">
		<rdfs:subClassOf rdf:resource="&fibo-md-dbtx-int;BondCoupon"/>
		<rdfs:subClassOf>
			<owl:Restriction>
				<owl:onProperty rdf:resource="&fibo-md-dbtx-int;projectedValue"/>
				<owl:someValuesFrom rdf:resource="&fibo-md-dbtx-int;ProjectedCouponPaymentValue"/>
			</owl:Restriction>
		</rdfs:subClassOf>
		<rdfs:label xml:lang="en">bond variable coupon</rdfs:label>
	</owl:Class>
	
	<owl:Class rdf:about="&fibo-md-dbtx-int;DebtInstrumentReferenceRate">
		<rdfs:subClassOf rdf:resource="https://spec.edmcouncil.org/fibo/IND/Indicators/Indicators/MarketRate"/>
		<rdfs:label xml:lang="en">debt instrument reference rate</rdfs:label>
		<skos:definition xml:lang="en">The interest rate of some debt instrument which is referred to in calculations of some sort.</skos:definition>
		<fibo-fnd-utl-av:explanatoryNote xml:lang="en">For example a US Treasury Bill interest Rate, used in quoting prices by way of spreads against this instrument. Also potentially an instrument the interest rate of which is used as the Base in a Floating Rate Note or other variable debt coupon formula.</fibo-fnd-utl-av:explanatoryNote>
	</owl:Class>
	
	<owl:Class rdf:about="&fibo-md-dbtx-int;DebtSecurityInterestAmount">
		<rdfs:subClassOf rdf:resource="&fibo-fnd-math-math;TimedParameter"/>
		<rdfs:label xml:lang="en">debt security interest amount</rdfs:label>
		<skos:definition xml:lang="en">The amount of interest paid out on a debt security at a given point in time.</skos:definition>
	</owl:Class>
	
	<owl:Class rdf:about="&fibo-md-dbtx-int;FRNCoupon">
		<rdfs:subClassOf rdf:resource="&fibo-md-dbtx-int;BondVariableCoupon"/>
		<rdfs:label xml:lang="en">f r n coupon</rdfs:label>
		<owl:disjointWith rdf:resource="&fibo-md-dbtx-int;IndexLinkedCoupon"/>
		<owl:disjointWith rdf:resource="&fibo-md-dbtx-int;InflationBondVariableCoupon"/>
		<owl:disjointWith rdf:resource="&fibo-md-dbtx-int;WACBondCoupon"/>
		<skos:definition xml:lang="en">Mechanism whereby an investor receives income from interest payments, which are usually made periodically. These are for a variable amount based on a specified Interest rate.</skos:definition>
	</owl:Class>
	
	<owl:Class rdf:about="&fibo-md-dbtx-int;IndexLinkedCoupon">
		<rdfs:subClassOf rdf:resource="&fibo-md-dbtx-int;BondVariableCoupon"/>
		<rdfs:label xml:lang="en">index linked coupon</rdfs:label>
		<owl:disjointWith rdf:resource="&fibo-md-dbtx-int;InflationBondVariableCoupon"/>
		<owl:disjointWith rdf:resource="&fibo-md-dbtx-int;WACBondCoupon"/>
	</owl:Class>
	
	<owl:Class rdf:about="&fibo-md-dbtx-int;InflationBondFactor">
		<rdfs:subClassOf rdf:resource="&fibo-md-temx-ins;ReferenceFactor"/>
		<rdfs:label xml:lang="en">inflation bond factor</rdfs:label>
		<skos:definition xml:lang="en">The factor which is used in determining the principal on an inflation bond. This is used either in calculating the interest payments, in calculating the principal payback or more typically both. Further notes: This is a dated parameter, that is it varies over time.</skos:definition>
	</owl:Class>
	
	<owl:Class rdf:about="&fibo-md-dbtx-int;InflationBondVariableCoupon">
		<rdfs:subClassOf rdf:resource="&fibo-md-dbtx-int;BondVariableCoupon"/>
		<rdfs:label xml:lang="en">inflation bond variable coupon</rdfs:label>
		<owl:disjointWith rdf:resource="&fibo-md-dbtx-int;WACBondCoupon"/>
	</owl:Class>
	
	<owl:Class rdf:about="&fibo-md-dbtx-int;ProjectedCouponPaymentValue">
		<rdfs:subClassOf rdf:resource="&fibo-fnd-math-math;ProjectedValue"/>
		<rdfs:label xml:lang="en">projected coupon payment value</rdfs:label>
		<skos:definition xml:lang="en">Projected Coupon amount, along with parameters defining when and how this is projected.</skos:definition>
	</owl:Class>
	
	<owl:Class rdf:about="&fibo-md-dbtx-int;TreasuryBillInterestRateValue">
		<rdfs:subClassOf rdf:resource="&fibo-fnd-math-math;TimedValue"/>
		<rdfs:label xml:lang="en">treasury bill interest rate value</rdfs:label>
		<skos:definition xml:lang="en">The value of a government short term debt security, or treasury bill, at a given point in time.</skos:definition>
	</owl:Class>
	
	<owl:Class rdf:about="&fibo-md-dbtx-int;TreasuryBillReferenceRate">
		<rdfs:subClassOf rdf:resource="&fibo-md-dbtx-int;DebtInstrumentReferenceRate"/>
		<rdfs:subClassOf>
			<owl:Restriction>
				<owl:onProperty rdf:resource="&fibo-md-dbtx-int;hasInterestRateValue"/>
				<owl:someValuesFrom rdf:resource="&fibo-md-dbtx-int;TreasuryBillInterestRateValue"/>
			</owl:Restriction>
		</rdfs:subClassOf>
		<rdfs:label xml:lang="en">treasury bill reference rate</rdfs:label>
		<skos:definition xml:lang="en">The parameter which is the interest rate payable by the T Bill at any point in time. This therefore takes a value at any given time and has historical values in the past.</skos:definition>
	</owl:Class>
	
	<owl:Class rdf:about="&fibo-md-dbtx-int;WACBondCoupon">
		<rdfs:subClassOf rdf:resource="&fibo-md-dbtx-int;BondVariableCoupon"/>
		<rdfs:label xml:lang="en">w a c bond coupon</rdfs:label>
	</owl:Class>
	
	<owl:ObjectProperty rdf:about="&fibo-md-dbtx-int;bondHasCoupon">
		<rdfs:label>bond has coupon</rdfs:label>
	</owl:ObjectProperty>
	
	<owl:ObjectProperty rdf:about="&fibo-md-dbtx-int;couponAmount">
		<rdfs:label xml:lang="en">coupon amount</rdfs:label>
		<rdfs:domain rdf:resource="&fibo-md-dbtx-int;BondVariableCoupon"/>
		<rdfs:range rdf:resource="&fibo-md-temx-tem;DatedPercentage"/>
		<skos:definition xml:lang="en">The current pr past amount of the bond coupon.</skos:definition>
	</owl:ObjectProperty>
	
	<owl:ObjectProperty rdf:about="&fibo-md-dbtx-int;hasFactor">
		<rdfs:label>has factor</rdfs:label>
	</owl:ObjectProperty>
	
	<owl:ObjectProperty rdf:about="&fibo-md-dbtx-int;hasInterestRateValue">
		<rdfs:subPropertyOf rdf:resource="&fibo-fnd-math-math;takesValuesOverTime"/>
		<rdfs:label xml:lang="en">has interest rate value</rdfs:label>
		<rdfs:domain rdf:resource="&fibo-md-dbtx-int;TreasuryBillReferenceRate"/>
		<rdfs:range rdf:resource="&fibo-md-dbtx-int;TreasuryBillInterestRateValue"/>
	</owl:ObjectProperty>
	
	<owl:ObjectProperty rdf:about="&fibo-md-dbtx-int;interestRate">
		<rdfs:label xml:lang="en">interest rate</rdfs:label>
		<rdfs:domain rdf:resource="&fibo-md-dbtx-int;TreasuryBillInterestRateValue"/>
		<rdfs:range rdf:resource="&fibo-fnd-utlx-val;PercentageValue"/>
		<skos:definition xml:lang="en">The rate of interest payable by the Treasury Bill at a stated time.</skos:definition>
	</owl:ObjectProperty>
	
	<owl:ObjectProperty rdf:about="&fibo-md-dbtx-int;projectedCoupon">
		<rdfs:label xml:lang="en">projected coupon</rdfs:label>
		<rdfs:domain rdf:resource="&fibo-md-dbtx-int;ProjectedCouponPaymentValue"/>
		<rdfs:range rdf:resource="&fibo-fnd-utlx-val;PercentageValue"/>
		<skos:definition xml:lang="en">Anticipated amount of a future (variable) coupon amount.</skos:definition>
	</owl:ObjectProperty>
	
	<owl:ObjectProperty rdf:about="&fibo-md-dbtx-int;projectedValue">
		<rdfs:label xml:lang="en">projected value</rdfs:label>
		<rdfs:domain rdf:resource="&fibo-md-dbtx-int;BondVariableCoupon"/>
		<rdfs:range rdf:resource="&fibo-md-dbtx-int;ProjectedCouponPaymentValue"/>
	</owl:ObjectProperty>

</rdf:RDF>