<?xml version="1.0" encoding="UTF-8"?>
<!DOCTYPE rdf:RDF [
	<!ENTITY dct "http://purl.org/dc/terms/">
	<!ENTITY fibo-fnd-dt-bd "https://spec.edmcouncil.org/fibo/ontology/FND/DatesAndTimes/BusinessDates/">
	<!ENTITY fibo-fnd-dt-fd "https://spec.edmcouncil.org/fibo/ontology/FND/DatesAndTimes/FinancialDates/">
	<!ENTITY fibo-fnd-plc-cty "https://spec.edmcouncil.org/fibo/ontology/FND/Places/Countries/">
	<!ENTITY fibo-fnd-rel-rel "https://spec.edmcouncil.org/fibo/ontology/FND/Relations/Relations/">
	<!ENTITY fibo-fnd-utl-av "https://spec.edmcouncil.org/fibo/ontology/FND/Utilities/AnnotationVocabulary/">
	<!ENTITY lcc-lr "https://www.omg.org/spec/LCC/Languages/LanguageRepresentation/">
	<!ENTITY owl "http://www.w3.org/2002/07/owl#">
	<!ENTITY rdf "http://www.w3.org/1999/02/22-rdf-syntax-ns#">
	<!ENTITY rdfs "http://www.w3.org/2000/01/rdf-schema#">
	<!ENTITY skos "http://www.w3.org/2004/02/skos/core#">
	<!ENTITY sm "http://www.omg.org/techprocess/ab/SpecificationMetadata/">
	<!ENTITY xsd "http://www.w3.org/2001/XMLSchema#">
]>
<rdf:RDF xml:base="https://spec.edmcouncil.org/fibo/ontology/FND/DatesAndTimes/BusinessDates/"
	xmlns:dct="http://purl.org/dc/terms/"
	xmlns:fibo-fnd-dt-bd="https://spec.edmcouncil.org/fibo/ontology/FND/DatesAndTimes/BusinessDates/"
	xmlns:fibo-fnd-dt-fd="https://spec.edmcouncil.org/fibo/ontology/FND/DatesAndTimes/FinancialDates/"
	xmlns:fibo-fnd-plc-cty="https://spec.edmcouncil.org/fibo/ontology/FND/Places/Countries/"
	xmlns:fibo-fnd-rel-rel="https://spec.edmcouncil.org/fibo/ontology/FND/Relations/Relations/"
	xmlns:fibo-fnd-utl-av="https://spec.edmcouncil.org/fibo/ontology/FND/Utilities/AnnotationVocabulary/"
	xmlns:lcc-lr="https://www.omg.org/spec/LCC/Languages/LanguageRepresentation/"
	xmlns:owl="http://www.w3.org/2002/07/owl#"
	xmlns:rdf="http://www.w3.org/1999/02/22-rdf-syntax-ns#"
	xmlns:rdfs="http://www.w3.org/2000/01/rdf-schema#"
	xmlns:skos="http://www.w3.org/2004/02/skos/core#"
	xmlns:sm="http://www.omg.org/techprocess/ab/SpecificationMetadata/"
	xmlns:xsd="http://www.w3.org/2001/XMLSchema#">
	
	<owl:Ontology rdf:about="https://spec.edmcouncil.org/fibo/ontology/FND/DatesAndTimes/BusinessDates/">
		<rdfs:label>Business Dates Ontology</rdfs:label>
		<dct:abstract>This ontology extends definitions of date and schedule concepts from the FinancialDates ontology with concepts defining dates that may be adjusted when they fall on weekends or holidays as defined in a given business center, for use in other FIBO ontologies.</dct:abstract>
		<dct:license rdf:datatype="&xsd;anyURI">http://opensource.org/licenses/MIT</dct:license>
		<sm:contentLanguage rdf:datatype="&xsd;anyURI">http://www.w3.org/standards/techs/owl#w3c_all</sm:contentLanguage>
		<sm:copyright>Copyright (c) 2014-2020 EDM Council, Inc.</sm:copyright>
		<sm:copyright>Copyright (c) 2014-2020 Object Management Group, Inc.</sm:copyright>
		<sm:dependsOn rdf:datatype="&xsd;anyURI">https://spec.edmcouncil.org/fibo/ontology/FND/DatesAndTimes/FinancialDates/</sm:dependsOn>
		<sm:dependsOn rdf:datatype="&xsd;anyURI">https://spec.edmcouncil.org/fibo/ontology/FND/Places/Countries/</sm:dependsOn>
		<sm:dependsOn rdf:datatype="&xsd;anyURI">https://spec.edmcouncil.org/fibo/ontology/FND/Relations/Relations/</sm:dependsOn>
		<sm:dependsOn rdf:datatype="&xsd;anyURI">https://spec.edmcouncil.org/fibo/ontology/FND/Utilities/AnnotationVocabulary/</sm:dependsOn>
		<sm:dependsOn rdf:datatype="&xsd;anyURI">https://www.omg.org/spec/LCC/</sm:dependsOn>
		<sm:fileAbbreviation>fibo-fnd-dt-bd</sm:fileAbbreviation>
		<sm:filename>BusinessDates.rdf</sm:filename>
		<owl:imports rdf:resource="https://spec.edmcouncil.org/fibo/ontology/FND/DatesAndTimes/FinancialDates/"/>
		<owl:imports rdf:resource="https://spec.edmcouncil.org/fibo/ontology/FND/Places/Countries/"/>
		<owl:imports rdf:resource="https://spec.edmcouncil.org/fibo/ontology/FND/Relations/Relations/"/>
		<owl:imports rdf:resource="https://spec.edmcouncil.org/fibo/ontology/FND/Utilities/AnnotationVocabulary/"/>
		<owl:imports rdf:resource="https://www.omg.org/spec/LCC/Languages/LanguageRepresentation/"/>
		<owl:versionIRI rdf:resource="https://spec.edmcouncil.org/fibo/ontology/FND/20200201/DatesAndTimes/BusinessDates/"/>
		<skos:changeNote>The https://spec.edmcouncil.org/fibo/ontology/FND/20141101/DatesAndTimes/BusinessDates/ version of this ontology was revised by the FIBO FND 1.2 RTF in order to add definitions for business recurrence intervals such as the day of the month and week, and to revise the representation of the end of the month to correspond to the way that the other intervals are represented for use in parametric schedules.</skos:changeNote>
		<skos:changeNote>The https://spec.edmcouncil.org/fibo/ontology/FND/20180801/DatesAndTimes/BusinessDates/ version of this ontology was revised to better support definitions related to business day adjustments.</skos:changeNote>
		<skos:changeNote>The https://spec.edmcouncil.org/fibo/ontology/FND/20180901/DatesAndTimes/BusinessDates/ version of this ontology was revised to loosen domains on properties related to business day and day count (recurrence interval) conventions, eliminate a duplicate individual, normalize definitions to be ISO 704 compliant, and eliminate duplication of concepts in LCC.</skos:changeNote>
		<skos:changeNote>This ontology was added to Foundations in advance of the December 2014 Long Beach meeting in support of the SEC specification.  It is also needed to provide temporal relationships for Ownership and Control.

These three ontologies are designed for use together:

   * FinancialDates  -- financial Dates and Schedules
   * BusinessDates -- business day adjustments
   * Occurrences    -- occurrences (events) and kinds of occurrences

They are modularized this way to minimize the ontological committments that are imposed upon ontologies that rely upon them.  Ontologies can import FinancialDates alone, or FinancialDates + BusinessDates, or FinancialDates + Occurrences, or all three together.</skos:changeNote>
		<fibo-fnd-utl-av:hasMaturityLevel rdf:resource="&fibo-fnd-utl-av;Release"/>
	</owl:Ontology>
	
	<owl:Class rdf:about="&fibo-fnd-dt-bd;BusinessDayAdjustment">
		<rdfs:subClassOf rdf:resource="&fibo-fnd-dt-bd;Convention"/>
		<rdfs:subClassOf>
			<owl:Restriction>
				<owl:onProperty rdf:resource="&fibo-fnd-dt-bd;hasBusinessDayConvention"/>
				<owl:onClass rdf:resource="&fibo-fnd-dt-bd;BusinessDayConvention"/>
				<owl:qualifiedCardinality rdf:datatype="&xsd;nonNegativeInteger">1</owl:qualifiedCardinality>
			</owl:Restriction>
		</rdfs:subClassOf>
		<rdfs:subClassOf>
			<owl:Restriction>
				<owl:onProperty rdf:resource="&fibo-fnd-dt-bd;hasBusinessCenter"/>
				<owl:someValuesFrom rdf:resource="&fibo-fnd-plc-cty;BusinessCenter"/>
			</owl:Restriction>
		</rdfs:subClassOf>
		<rdfs:label>business day adjustment</rdfs:label>
		<skos:definition>convention that specifies what happens when a date falls on a day that is a weekend or a holiday in one or more business centers</skos:definition>
	</owl:Class>
	
	<owl:Class rdf:about="&fibo-fnd-dt-bd;BusinessDayConvention">
		<rdfs:subClassOf rdf:resource="&fibo-fnd-dt-bd;Convention"/>
		<rdfs:label>business day convention</rdfs:label>
		<skos:definition>convention that enumerates the possible ways to handle a date that falls on a weekend or holiday</skos:definition>
	</owl:Class>
	
	<owl:NamedIndividual rdf:about="&fibo-fnd-dt-bd;BusinessDayFollowing">
		<rdf:type rdf:resource="&fibo-fnd-dt-bd;BusinessDayConvention"/>
		<rdfs:label>business day following</rdfs:label>
		<sm:normativeReference>FPML 5.1 &quot;BusinessDayConventionEnum&quot;</sm:normativeReference>
		<skos:definition>convention specifying that a non-business date will be adjusted to the first following day that is a business day</skos:definition>
	</owl:NamedIndividual>
	
	<owl:NamedIndividual rdf:about="&fibo-fnd-dt-bd;BusinessDayModifiedFollowing">
		<rdf:type rdf:resource="&fibo-fnd-dt-bd;BusinessDayConvention"/>
		<rdfs:label>business day modified following</rdfs:label>
		<sm:normativeReference>FPML 5.1 &quot;BusinessDayConventionEnum&quot;</sm:normativeReference>
		<skos:definition>convention specifying that a non-business date will be adjusted to the first following day that is a business day unless that day falls in the next calendar month, in which case that date will be the first preceding day that is a calendar date</skos:definition>
	</owl:NamedIndividual>
	
	<owl:NamedIndividual rdf:about="&fibo-fnd-dt-bd;BusinessDayModifiedPreceding">
		<rdf:type rdf:resource="&fibo-fnd-dt-bd;BusinessDayConvention"/>
		<rdfs:label>business day modified preceding</rdfs:label>
		<sm:normativeReference>FPML 5.1 &quot;BusinessDayConventionEnum&quot;</sm:normativeReference>
		<skos:definition>convention specifying that a non-business date will be adjusted to the first preceding day that is a business day unless that day falls in the previous month, in which case that date will be the first following day that is a business day</skos:definition>
	</owl:NamedIndividual>
	
	<owl:NamedIndividual rdf:about="&fibo-fnd-dt-bd;BusinessDayNearest">
		<rdf:type rdf:resource="&fibo-fnd-dt-bd;BusinessDayConvention"/>
		<rdfs:label>business day nearest</rdfs:label>
		<sm:normativeReference>FPML 5.1 &quot;BusinessDayConventionEnum&quot;</sm:normativeReference>
		<skos:definition>convention specifying that a non-business date will be adjusted to the nearest day that is a business day -- i.e. if the non-business day falls on any day other than a Sunday or a Monday, it will be the first preceding day that is a business day, and will be the first following business day if it falls on a Sunday or a Monday</skos:definition>
	</owl:NamedIndividual>
	
	<owl:NamedIndividual rdf:about="&fibo-fnd-dt-bd;BusinessDayNone">
		<rdf:type rdf:resource="&fibo-fnd-dt-bd;BusinessDayConvention"/>
		<rdfs:label>business day none</rdfs:label>
		<sm:normativeReference>FPML 5.1 &quot;BusinessDayConventionEnum&quot;</sm:normativeReference>
		<skos:definition>convention specifying that a date will not be adjusted if it falls on a day that is not a business day</skos:definition>
	</owl:NamedIndividual>
	
	<owl:NamedIndividual rdf:about="&fibo-fnd-dt-bd;BusinessDayPreceding">
		<rdf:type rdf:resource="&fibo-fnd-dt-bd;BusinessDayConvention"/>
		<rdfs:label>business day preceding</rdfs:label>
		<skos:definition>convention specifying that a date will be adjusted to the first previous day that is a business day</skos:definition>
	</owl:NamedIndividual>
	
	<owl:Class rdf:about="&fibo-fnd-dt-bd;BusinessRecurrenceInterval">
		<rdfs:subClassOf rdf:resource="&fibo-fnd-dt-fd;RecurrenceInterval"/>
		<rdfs:subClassOf>
			<owl:Restriction>
				<owl:onProperty rdf:resource="&fibo-fnd-dt-bd;hasBusinessRecurrenceIntervalConvention"/>
				<owl:onClass rdf:resource="&fibo-fnd-dt-bd;BusinessRecurrenceIntervalConvention"/>
				<owl:qualifiedCardinality rdf:datatype="&xsd;nonNegativeInteger">1</owl:qualifiedCardinality>
			</owl:Restriction>
		</rdfs:subClassOf>
		<rdfs:label>business recurrence interval</rdfs:label>
		<skos:definition>recurrence interval that is specified using a business recurrence interval convention</skos:definition>
	</owl:Class>
	
	<owl:Class rdf:about="&fibo-fnd-dt-bd;BusinessRecurrenceIntervalConvention">
		<rdfs:subClassOf rdf:resource="&fibo-fnd-dt-bd;Convention"/>
		<rdfs:label>business recurrence interval convention</rdfs:label>
		<skos:definition>convention that specifies how recurring days should be handled, such as the end of the month, a particular day of the month, a day of the week, or more specifically, a t-bill auction date</skos:definition>
	</owl:Class>
	
	<owl:Class rdf:about="&fibo-fnd-dt-bd;Convention">
		<rdfs:label>convention</rdfs:label>
		<skos:definition>widely accepted or established way of doing &apos;something&apos; within some community of practice</skos:definition>
		<fibo-fnd-utl-av:adaptedFrom>Barron&apos;s Dictionary of Business and Economics Terms, Fifth Edition, 2012</fibo-fnd-utl-av:adaptedFrom>
		<fibo-fnd-utl-av:adaptedFrom rdf:datatype="&xsd;anyURI">https://en.oxforddictionaries.com/definition/convention</fibo-fnd-utl-av:adaptedFrom>
	</owl:Class>
	
	<owl:Class rdf:about="&fibo-fnd-dt-bd;DayOfMonth">
		<rdfs:subClassOf rdf:resource="&fibo-fnd-dt-bd;BusinessRecurrenceInterval"/>
		<rdfs:subClassOf>
			<owl:Restriction>
				<owl:onProperty rdf:resource="&fibo-fnd-dt-fd;hasOrdinalNumber"/>
				<owl:onDataRange rdf:resource="&xsd;nonNegativeInteger"/>
				<owl:qualifiedCardinality rdf:datatype="&xsd;nonNegativeInteger">1</owl:qualifiedCardinality>
			</owl:Restriction>
		</rdfs:subClassOf>
		<rdfs:label>day of month</rdfs:label>
		<skos:definition>specific, recurring day of the month</skos:definition>
	</owl:Class>
	
	<owl:Class rdf:about="&fibo-fnd-dt-bd;DayOfWeek">
		<rdfs:subClassOf rdf:resource="&fibo-fnd-dt-bd;BusinessRecurrenceInterval"/>
		<rdfs:label>day of the week</rdfs:label>
		<owl:equivalentClass>
			<owl:Class>
				<owl:oneOf rdf:parseType="Collection">
					<rdf:Description rdf:about="&fibo-fnd-dt-fd;Monday">
					</rdf:Description>
					<rdf:Description rdf:about="&fibo-fnd-dt-fd;Tuesday">
					</rdf:Description>
					<rdf:Description rdf:about="&fibo-fnd-dt-fd;Wednesday">
					</rdf:Description>
					<rdf:Description rdf:about="&fibo-fnd-dt-fd;Thursday">
					</rdf:Description>
					<rdf:Description rdf:about="&fibo-fnd-dt-fd;Friday">
					</rdf:Description>
					<rdf:Description rdf:about="&fibo-fnd-dt-fd;Saturday">
					</rdf:Description>
					<rdf:Description rdf:about="&fibo-fnd-dt-fd;Sunday">
					</rdf:Description>
				</owl:oneOf>
			</owl:Class>
		</owl:equivalentClass>
		<skos:definition>specific, recurring day of the week</skos:definition>
	</owl:Class>
	
	<owl:Class rdf:about="&fibo-fnd-dt-bd;EndOfMonth">
		<rdfs:subClassOf rdf:resource="&fibo-fnd-dt-bd;BusinessRecurrenceInterval"/>
		<rdfs:label>end of the month</rdfs:label>
		<skos:definition>the last day of a calendar month, irrespective of the length of the calendar month</skos:definition>
	</owl:Class>
	
	<owl:ObjectProperty rdf:about="&fibo-fnd-dt-bd;hasBusinessCenter">
		<rdfs:subPropertyOf rdf:resource="&lcc-lr;has"/>
		<rdfs:label>has business center</rdfs:label>
		<rdfs:range rdf:resource="&fibo-fnd-plc-cty;BusinessCenter"/>
		<skos:definition>identifies a location where business is conducted, and hence the business calendar used to adjust dates</skos:definition>
	</owl:ObjectProperty>
	
	<owl:ObjectProperty rdf:about="&fibo-fnd-dt-bd;hasBusinessDayAdjustment">
		<rdfs:subPropertyOf rdf:resource="&lcc-lr;has"/>
		<rdfs:label>has business day adjustment</rdfs:label>
		<rdfs:range rdf:resource="&fibo-fnd-dt-bd;BusinessDayAdjustment"/>
		<skos:definition>identifies a convention for adjustment of the business day for handling weekends and holidays</skos:definition>
	</owl:ObjectProperty>
	
	<owl:ObjectProperty rdf:about="&fibo-fnd-dt-bd;hasBusinessDayConvention">
		<rdfs:subPropertyOf rdf:resource="&lcc-lr;has"/>
		<rdfs:label>has business day convention</rdfs:label>
		<rdfs:range rdf:resource="&fibo-fnd-dt-bd;BusinessDayConvention"/>
		<skos:definition>identifies a convention regarding how a date should be handled when it falls on a day that is not a business day</skos:definition>
	</owl:ObjectProperty>
	
	<owl:ObjectProperty rdf:about="&fibo-fnd-dt-bd;hasBusinessRecurrenceIntervalConvention">
		<rdfs:subPropertyOf rdf:resource="&lcc-lr;has"/>
		<rdfs:label>has business recurrence interval convention</rdfs:label>
		<rdfs:range rdf:resource="&fibo-fnd-dt-bd;BusinessRecurrenceIntervalConvention"/>
		<skos:definition>identifies a convention regarding how certain recurring dates should be handled with respect to a given schedule, such as the end of the month</skos:definition>
	</owl:ObjectProperty>
	
	<owl:ObjectProperty rdf:about="&fibo-fnd-dt-bd;holdsDuring">
		<rdfs:subPropertyOf rdf:resource="&fibo-fnd-dt-fd;hasDatePeriod"/>
		<rdfs:label>holds during</rdfs:label>
		<skos:definition>specifies that some condition or state is true (holds) during a specified date period</skos:definition>
	</owl:ObjectProperty>
	
	<owl:Class rdf:about="&fibo-fnd-dt-fd;CalculatedDate">
		<rdfs:subClassOf>
			<owl:Restriction>
				<owl:onProperty rdf:resource="&fibo-fnd-dt-bd;hasBusinessDayAdjustment"/>
				<owl:onClass rdf:resource="&fibo-fnd-dt-bd;BusinessDayAdjustment"/>
				<owl:maxQualifiedCardinality rdf:datatype="&xsd;nonNegativeInteger">1</owl:maxQualifiedCardinality>
			</owl:Restriction>
		</rdfs:subClassOf>
	</owl:Class>
	
	<owl:Class rdf:about="&fibo-fnd-dt-fd;RegularSchedule">
		<rdfs:subClassOf>
			<owl:Restriction>
				<owl:onProperty rdf:resource="&fibo-fnd-dt-bd;hasBusinessDayAdjustment"/>
				<owl:onClass rdf:resource="&fibo-fnd-dt-bd;BusinessDayAdjustment"/>
				<owl:maxQualifiedCardinality rdf:datatype="&xsd;nonNegativeInteger">1</owl:maxQualifiedCardinality>
			</owl:Restriction>
		</rdfs:subClassOf>
	</owl:Class>

</rdf:RDF>