<?xml version="1.0" encoding="UTF-8"?>
<!DOCTYPE rdf:RDF [
	<!ENTITY dct "http://purl.org/dc/terms/">
	<!ENTITY fibo-fnd-arr-arr "https://spec.edmcouncil.org/fibo/FND/Arrangements/Arrangements/">
	<!ENTITY fibo-fnd-dt-fd "https://spec.edmcouncil.org/fibo/FND/DatesAndTimes/FinancialDates/">
	<!ENTITY fibo-fnd-plc-loc "https://spec.edmcouncil.org/fibo/FND/Places/Locations/">
	<!ENTITY fibo-fnd-rel-rel "https://spec.edmcouncil.org/fibo/FND/Relations/Relations/">
	<!ENTITY fibo-fnd-utl-av "https://spec.edmcouncil.org/fibo/FND/Utilities/AnnotationVocabulary/">
	<!ENTITY owl "http://www.w3.org/2002/07/owl#">
	<!ENTITY rdf "http://www.w3.org/1999/02/22-rdf-syntax-ns#">
	<!ENTITY rdfs "http://www.w3.org/2000/01/rdf-schema#">
	<!ENTITY skos "http://www.w3.org/2004/02/skos/core#">
	<!ENTITY sm "http://www.omg.org/techprocess/ab/SpecificationMetadata/">
	<!ENTITY xsd "http://www.w3.org/2001/XMLSchema#">
]>
<rdf:RDF xml:base="https://spec.edmcouncil.org/fibo/FND/DatesAndTimes/FinancialDates/"
	xmlns:dct="http://purl.org/dc/terms/"
	xmlns:fibo-fnd-arr-arr="https://spec.edmcouncil.org/fibo/FND/Arrangements/Arrangements/"
	xmlns:fibo-fnd-dt-fd="https://spec.edmcouncil.org/fibo/FND/DatesAndTimes/FinancialDates/"
	xmlns:fibo-fnd-plc-loc="https://spec.edmcouncil.org/fibo/FND/Places/Locations/"
	xmlns:fibo-fnd-rel-rel="https://spec.edmcouncil.org/fibo/FND/Relations/Relations/"
	xmlns:fibo-fnd-utl-av="https://spec.edmcouncil.org/fibo/FND/Utilities/AnnotationVocabulary/"
	xmlns:owl="http://www.w3.org/2002/07/owl#"
	xmlns:rdf="http://www.w3.org/1999/02/22-rdf-syntax-ns#"
	xmlns:rdfs="http://www.w3.org/2000/01/rdf-schema#"
	xmlns:skos="http://www.w3.org/2004/02/skos/core#"
	xmlns:sm="http://www.omg.org/techprocess/ab/SpecificationMetadata/"
	xmlns:xsd="http://www.w3.org/2001/XMLSchema#">
	
	<owl:Ontology rdf:about="https://spec.edmcouncil.org/fibo/FND/DatesAndTimes/FinancialDates/">
		<rdfs:label>Financial Dates Ontology</rdfs:label>
		<dct:license rdf:datatype="&xsd;anyURI">http://www.omg.org/techprocess/ab/SpecificationMetadata/MITLicense</dct:license>
		<sm:contentLanguage rdf:datatype="&xsd;anyURI">http://www.omg.org/spec/ODM/</sm:contentLanguage>
		<sm:contentLanguage rdf:datatype="&xsd;anyURI">http://www.w3.org/standards/techs/owl#w3c_all</sm:contentLanguage>
		<sm:copyright>Copyright (c) 2014-2017 EDM Council, Inc.
Copyright (c) 2014-2017 Object Management Group, Inc.</sm:copyright>
		<sm:dependsOn rdf:datatype="&xsd;anyURI">https://spec.edmcouncil.org/fibo/FND/Arrangements/Arrangements/</sm:dependsOn>
		<sm:dependsOn rdf:datatype="&xsd;anyURI">https://spec.edmcouncil.org/fibo/FND/Places/Locations/</sm:dependsOn>
		<sm:dependsOn rdf:datatype="&xsd;anyURI">https://spec.edmcouncil.org/fibo/FND/Relations/Relations/</sm:dependsOn>
		<sm:dependsOn rdf:datatype="&xsd;anyURI">https://spec.edmcouncil.org/fibo/FND/Utilities/AnnotationVocabulary/</sm:dependsOn>
		<sm:fileAbbreviation>fibo-fnd-dt-fd</sm:fileAbbreviation>
		<sm:fileAbstract>This ontology provides definitions of date and schedule concepts for use in other FIBO ontologies.</sm:fileAbstract>
		<sm:filename>FinancialDates.rdf</sm:filename>
		<rdfs:seeAlso rdf:resource="https://spec.edmcouncil.org/fibo/AboutTheEDMC-FIBOFamily/"/>
		<rdfs:seeAlso rdf:resource="https://spec.edmcouncil.org/fibo/FND/AboutFND/"/>
		<rdfs:seeAlso rdf:resource="https://spec.edmcouncil.org/fibo/FND/DatesAndTimes/AboutDatesAndTimes/"/>
		<owl:imports rdf:resource="https://spec.edmcouncil.org/fibo/FND/Arrangements/Arrangements/"/>
		<owl:imports rdf:resource="https://spec.edmcouncil.org/fibo/FND/Places/Locations/"/>
		<owl:imports rdf:resource="https://spec.edmcouncil.org/fibo/FND/Relations/Relations/"/>
		<owl:imports rdf:resource="https://spec.edmcouncil.org/fibo/FND/Utilities/AnnotationVocabulary/"/>
		<owl:versionIRI rdf:resource="https://spec.edmcouncil.org/fibo/FND/20170801/DatesAndTimes/FinancialDates/"/>
		<skos:changeNote>The https://spec.edmcouncil.org/fibo/FND/20141101/DatesAndTimes/FinancialDates/ version of this ontology was revised by the FIBO FND 1.2 RTF in order to introduce the definition of a time interval, which is a location, to ground some of the concepts such as a date period, and duration as well as to support the definition of business recurrence intervals for use in parametric schedules for securities.</skos:changeNote>
		<skos:changeNote>The https://spec.edmcouncil.org/fibo/FND/20170201/DatesAndTimes/FinancialDates/ version of this ontology was revised by the FIBO FND 1.3 RTF in order to introduce the definition of a time instant, to eliminate a reasoning issue with relative dates, and remove a circular dependency inadvertently incorporated in the ontology with a FIBO FND 1.2 modification.</skos:changeNote>
		<skos:changeNote>This ontology was added to Foundations in advance of the December 2014 Long Beach meeting in support of the SEC specification.  It is also needed to provide temporal relationships for Ownership and Control.

These three ontologies are designed for use together:

   * FinancialDates  -- financial Dates and Schedules
   * BusinessDates -- business day adjustments
   * Occurrences    -- occurrences (events) and kinds of occurrences

They are modularized this way to minimize the ontological committments that are imposed upon ontologies that rely upon them.  Ontologies can import FinancialDates alone, or FinancialDates + BusinessDates, or FinancialDates + Occurrences, or all three together.</skos:changeNote>
		<fibo-fnd-utl-av:hasMaturityLevel rdf:resource="&fibo-fnd-utl-av;Release"/>
	</owl:Ontology>
	
	<owl:Class rdf:about="&fibo-fnd-dt-fd;AdHocSchedule">
		<rdfs:subClassOf rdf:resource="&fibo-fnd-dt-fd;Schedule"/>
		<rdfs:subClassOf>
			<owl:Restriction>
				<owl:onProperty rdf:resource="&fibo-fnd-rel-rel;comprises"/>
				<owl:someValuesFrom rdf:resource="&fibo-fnd-dt-fd;AdHocScheduleEntry"/>
			</owl:Restriction>
		</rdfs:subClassOf>
		<rdfs:label>ad hoc schedule</rdfs:label>
		<skos:definition>a schedule that consists of (comprises) AdHocScheduleEntries, each of which specifies a date</skos:definition>
		<fibo-fnd-utl-av:usageNote>Other ontologies can extend AdHocSchedule and/or AdHocScheduleEntry as needed to relate the date to something. In particular, the Occurrences ontology extends AdHocScheduleEntry to associate an OccurrenceKind with each entry. The intended meaning is that an Occurrence of the OccurrenceKind happens on the corresponding Date.</fibo-fnd-utl-av:usageNote>
	</owl:Class>
	
	<owl:Class rdf:about="&fibo-fnd-dt-fd;AdHocScheduleEntry">
		<rdfs:subClassOf>
			<owl:Restriction>
				<owl:onProperty rdf:resource="&fibo-fnd-dt-fd;hasDate"/>
				<owl:onClass rdf:resource="&fibo-fnd-dt-fd;Date"/>
				<owl:qualifiedCardinality rdf:datatype="&xsd;nonNegativeInteger">1</owl:qualifiedCardinality>
			</owl:Restriction>
		</rdfs:subClassOf>
		<rdfs:label>ad hoc schedule entry</rdfs:label>
		<skos:definition>an entry, including a date, among multiple ad hoc schedule entries that jointly make up an AdHocSchedule</skos:definition>
		<fibo-fnd-utl-av:usageNote>Other ontologies can extend AdHocScheduleEntry as needed. In particular, the Occurrences ontology extends AdHocScheduleEntry to comprise an OccurrenceKind. The meaning is that an ad hoc schedule entry comprises a date and an event which is scheduled to occur on that date; in other words Occurrence of the OccurrenceKind should happen on the Date of the OccurrenceKind.</fibo-fnd-utl-av:usageNote>
		<fibo-fnd-utl-av:usageNote>The Date of an AdHocScheduleEntry can be an ExplicitDate or any kind of CalculatedDate, such as:

* An OccurrenceBasedDate -- a Date that itself is defined by an Occurrence (see the Occurrences ontology)
* A RelativeDate - a Date relative to another Date, such as T+3
* A SpecifiedDate - a Date that is defined by an arbitrary rule</fibo-fnd-utl-av:usageNote>
	</owl:Class>
	
	<owl:Class rdf:about="&fibo-fnd-dt-fd;CalculatedDate">
		<rdfs:subClassOf rdf:resource="&fibo-fnd-dt-fd;Date"/>
		<rdfs:label>calculated date</rdfs:label>
		<owl:disjointWith rdf:resource="&fibo-fnd-dt-fd;ExplicitDate"/>
		<skos:definition>a date that is or will be calculated in some way</skos:definition>
		<fibo-fnd-utl-av:explanatoryNote>The hasDateValue property of a CalculatedDate is not set until the Date is calculated.  Since the calculation may depend upon future events that may or may not ever happen, the hasDateValue property may never be set.</fibo-fnd-utl-av:explanatoryNote>
	</owl:Class>
	
	<fibo-fnd-dt-fd:CalendarPeriod rdf:about="&fibo-fnd-dt-fd;CalendarMonth">
		<rdf:type rdf:resource="&owl;NamedIndividual"/>
		<rdfs:label>calendar month</rdfs:label>
		<sm:normativeReference>ISO 8601, clause 2.2.11</sm:normativeReference>
		<skos:definition>time interval resulting from the division of a calendar year in 12 time intervals, each with a specific name and containing a specific number of calendar days</skos:definition>
	</fibo-fnd-dt-fd:CalendarPeriod>
	
	<owl:Class rdf:about="&fibo-fnd-dt-fd;CalendarPeriod">
		<rdfs:subClassOf rdf:resource="&fibo-fnd-dt-fd;TimeInterval"/>
		<rdfs:label>calendar period</rdfs:label>
		<skos:definition>an enumeration that indicates whether a CalendarSpecifiedDate is figured with respect to a calendar week, a calendar month, a calendar quarter, or a calendar year</skos:definition>
		<skos:editorialNote>The terms &apos;calendar xxx&apos; are intended to reinforce that these are periods on a calendar, not durations. 

For example, a calendar year always starts on a January 1 and ends on a December 31. The term &apos;calendar year&apos; does not mean the same thing as  a duration (an amount of time) of 1 year, nor can a calendar year start on any arbitrary day of a year.  For example, a calendar year never starts on September 1.

Similar points apply to other kinds of calendar periods, such as calendar week, calendar month, and calendar quarter.</skos:editorialNote>
	</owl:Class>
	
	<fibo-fnd-dt-fd:CalendarPeriod rdf:about="&fibo-fnd-dt-fd;CalendarQuarter">
		<rdf:type rdf:resource="&owl;NamedIndividual"/>
		<rdfs:label>calendar quarter</rdfs:label>
		<skos:definition>time interval of 3 months, starting on January 1, April 1, July 1, or October 1</skos:definition>
	</fibo-fnd-dt-fd:CalendarPeriod>
	
	<owl:Class rdf:about="&fibo-fnd-dt-fd;CalendarSpecifiedInterval">
		<rdfs:subClassOf rdf:resource="&fibo-fnd-dt-fd;RecurrenceInterval"/>
		<rdfs:subClassOf>
			<owl:Restriction>
				<owl:onProperty rdf:resource="&fibo-fnd-dt-fd;hasCalendarPeriod"/>
				<owl:onClass rdf:resource="&fibo-fnd-dt-fd;CalendarPeriod"/>
				<owl:qualifiedCardinality rdf:datatype="&xsd;nonNegativeInteger">1</owl:qualifiedCardinality>
			</owl:Restriction>
		</rdfs:subClassOf>
		<rdfs:subClassOf>
			<owl:Restriction>
				<owl:onProperty rdf:resource="&fibo-fnd-dt-fd;hasTimeDirection"/>
				<owl:onClass rdf:resource="&fibo-fnd-dt-fd;TimeDirection"/>
				<owl:qualifiedCardinality rdf:datatype="&xsd;nonNegativeInteger">1</owl:qualifiedCardinality>
			</owl:Restriction>
		</rdfs:subClassOf>
		<rdfs:subClassOf>
			<owl:Restriction>
				<owl:onProperty rdf:resource="&fibo-fnd-dt-fd;hasOrdinalNumber"/>
				<owl:onDataRange rdf:resource="&xsd;integer"/>
				<owl:qualifiedCardinality rdf:datatype="&xsd;nonNegativeInteger">1</owl:qualifiedCardinality>
			</owl:Restriction>
		</rdfs:subClassOf>
		<rdfs:label>calendar specified interval</rdfs:label>
		<owl:disjointWith rdf:resource="&fibo-fnd-dt-fd;ExplicitRecurrenceInterval"/>
		<skos:definition>a RecurrenceInterval that is specified as the nth day of some CalendarPeriod (such as a calendar month), and a TimeDirection (forward from the beginning of the month, or backwards from the end).

The nth day is an ordinal number, not a cardinal number. &apos;1&apos; means the first day of the calendar period.</skos:definition>
		<skos:example>The 15th day of each calendar month.</skos:example>
		<skos:example>The last day of each quarter, specified as RelativeDay 1, and TimeDirection set to FromEnd.</skos:example>
	</owl:Class>
	
	<fibo-fnd-dt-fd:CalendarPeriod rdf:about="&fibo-fnd-dt-fd;CalendarWeek">
		<rdf:type rdf:resource="&owl;NamedIndividual"/>
		<rdfs:label>calendar week</rdfs:label>
		<sm:normativeReference>ISO 8601, clause 2.2.8</sm:normativeReference>
		<skos:definition>time interval of seven calendar days starting on a Monday</skos:definition>
	</fibo-fnd-dt-fd:CalendarPeriod>
	
	<fibo-fnd-dt-fd:CalendarPeriod rdf:about="&fibo-fnd-dt-fd;CalendarYear">
		<rdf:type rdf:resource="&owl;NamedIndividual"/>
		<rdfs:label>calendar year</rdfs:label>
		<sm:normativeReference>ISO 8601 clause 2.2.13</sm:normativeReference>
		<skos:definition>cyclic time interval in a calendar which is required for one revolution of the Earth around the Sun and approximated to an integral number of calendar days; a year in the Gregorian calendar</skos:definition>
	</fibo-fnd-dt-fd:CalendarPeriod>
	
	<owl:Class rdf:about="&fibo-fnd-dt-fd;Date">
		<rdfs:subClassOf>
			<owl:Restriction>
				<owl:onProperty rdf:resource="&fibo-fnd-dt-fd;hasDateValue"/>
				<owl:maxQualifiedCardinality rdf:datatype="&xsd;nonNegativeInteger">1</owl:maxQualifiedCardinality>
				<owl:onDataRange rdf:resource="&xsd;string"/>
			</owl:Restriction>
		</rdfs:subClassOf>
		<rdfs:label>date</rdfs:label>
		<skos:definition>a calendar day on some calendar</skos:definition>
		<fibo-fnd-utl-av:usageNote>A Date may or may not have a value, and may be explicit or calculated. A Date that has a value is one that is either explicitly set as a literal when it is created, or is some form of CalculatedDate.  In an instance of Date, the existence of the &apos;hasDateValue&apos; property both indicates that the Date is known, and gives the value of the Date. A Date that does not have a value is one that is some form of CalculatedDate, in which the actual date has not (yet) been established.</fibo-fnd-utl-av:usageNote>
	</owl:Class>
	
	<owl:Class rdf:about="&fibo-fnd-dt-fd;DatePeriod">
		<rdfs:subClassOf rdf:resource="&fibo-fnd-dt-fd;TimeInterval"/>
		<rdfs:subClassOf>
			<owl:Restriction>
				<owl:onProperty rdf:resource="&fibo-fnd-dt-fd;hasEndDate"/>
				<owl:onClass rdf:resource="&fibo-fnd-dt-fd;Date"/>
				<owl:maxQualifiedCardinality rdf:datatype="&xsd;nonNegativeInteger">1</owl:maxQualifiedCardinality>
			</owl:Restriction>
		</rdfs:subClassOf>
		<rdfs:subClassOf>
			<owl:Restriction>
				<owl:onProperty rdf:resource="&fibo-fnd-dt-fd;hasStartDate"/>
				<owl:onClass rdf:resource="&fibo-fnd-dt-fd;Date"/>
				<owl:maxQualifiedCardinality rdf:datatype="&xsd;nonNegativeInteger">1</owl:maxQualifiedCardinality>
			</owl:Restriction>
		</rdfs:subClassOf>
		<rdfs:subClassOf>
			<owl:Restriction>
				<owl:onProperty rdf:resource="&fibo-fnd-dt-fd;hasDuration"/>
				<owl:onClass rdf:resource="&fibo-fnd-dt-fd;Duration"/>
				<owl:maxQualifiedCardinality rdf:datatype="&xsd;nonNegativeInteger">1</owl:maxQualifiedCardinality>
			</owl:Restriction>
		</rdfs:subClassOf>
		<rdfs:label>date period</rdfs:label>
		<skos:definition>a time span over one or more calendar days, defined by at least two of three properties: (1) a start date, (2) an end date, and (3) a date period (duration); if more than one of these properties is missing, the DatePeriod is invalid</skos:definition>
		<fibo-fnd-utl-av:usageNote>A DatePeriod is unknown if either the startDate or the endDate has no value. If a DatePeriod is unknown, then the duration should either be omitted or unknown (have no value).</fibo-fnd-utl-av:usageNote>
	</owl:Class>
	
	<owl:Class rdf:about="&fibo-fnd-dt-fd;DateTime">
		<rdfs:subClassOf>
			<owl:Restriction>
				<owl:onProperty rdf:resource="&fibo-fnd-dt-fd;hasDateTimeValue"/>
				<owl:maxQualifiedCardinality rdf:datatype="&xsd;nonNegativeInteger">1</owl:maxQualifiedCardinality>
				<owl:onDataRange rdf:resource="&xsd;dateTime"/>
			</owl:Restriction>
		</rdfs:subClassOf>
		<rdfs:label>date time</rdfs:label>
		<skos:definition>a combination of a date and a time, without a time zone</skos:definition>
		<fibo-fnd-utl-av:usageNote>&apos;hasDateTimeValue&apos; is omitted if the DateTime is not (yet) known.</fibo-fnd-utl-av:usageNote>
		<fibo-fnd-utl-av:usageNote>Use DateTime for the combination of a Date and a time, without a time zone. Use DateTimeStamp for the combination of a Date and a time and a time zone.</fibo-fnd-utl-av:usageNote>
	</owl:Class>
	
	<owl:Class rdf:about="&fibo-fnd-dt-fd;DateTimeStamp">
		<rdfs:subClassOf>
			<owl:Restriction>
				<owl:onProperty rdf:resource="&fibo-fnd-dt-fd;hasDateTimeStampValue"/>
				<owl:maxQualifiedCardinality rdf:datatype="&xsd;nonNegativeInteger">1</owl:maxQualifiedCardinality>
				<owl:onDataRange rdf:resource="&xsd;dateTimeStamp"/>
			</owl:Restriction>
		</rdfs:subClassOf>
		<rdfs:label>date time stamp</rdfs:label>
		<skos:definition>a combination of a date, a time, and a time zone</skos:definition>
		<fibo-fnd-utl-av:synonym>time stamp</fibo-fnd-utl-av:synonym>
		<fibo-fnd-utl-av:usageNote>&apos;hasDateTimeStampValue&apos; is omitted if the DateTimeStamp is not (yet) established.</fibo-fnd-utl-av:usageNote>
		<fibo-fnd-utl-av:usageNote>Use DateTimeStamp when the time stamp includes a time zone field. Use DateTime for the combination of a Date and a time, without a time zone.</fibo-fnd-utl-av:usageNote>
	</owl:Class>
	
	<owl:Class rdf:about="&fibo-fnd-dt-fd;Duration">
		<rdfs:subClassOf rdf:resource="&fibo-fnd-dt-fd;TimeInterval"/>
		<rdfs:subClassOf>
			<owl:Restriction>
				<owl:onProperty rdf:resource="&fibo-fnd-dt-fd;hasDurationValue"/>
				<owl:maxQualifiedCardinality rdf:datatype="&xsd;nonNegativeInteger">1</owl:maxQualifiedCardinality>
				<owl:onDataRange rdf:resource="&xsd;string"/>
			</owl:Restriction>
		</rdfs:subClassOf>
		<rdfs:label>duration</rdfs:label>
		<skos:definition>an interval of time of some specific length</skos:definition>
		<fibo-fnd-utl-av:usageNote>The &apos;hasDurationValue&apos; property is absent if the duration is not (yet) known.</fibo-fnd-utl-av:usageNote>
	</owl:Class>
	
	<owl:Class rdf:about="&fibo-fnd-dt-fd;ExplicitDate">
		<rdfs:subClassOf rdf:resource="&fibo-fnd-dt-fd;Date"/>
		<rdfs:subClassOf>
			<owl:Restriction>
				<owl:onProperty rdf:resource="&fibo-fnd-dt-fd;hasDateValue"/>
				<owl:onDataRange rdf:resource="&xsd;string"/>
				<owl:qualifiedCardinality rdf:datatype="&xsd;nonNegativeInteger">1</owl:qualifiedCardinality>
			</owl:Restriction>
		</rdfs:subClassOf>
		<rdfs:label>explicit date</rdfs:label>
		<skos:definition>a date in which the &apos;hasDateValue&apos; property is required</skos:definition>
	</owl:Class>
	
	<owl:Class rdf:about="&fibo-fnd-dt-fd;ExplicitDatePeriod">
		<rdfs:subClassOf rdf:resource="&fibo-fnd-dt-fd;DatePeriod"/>
		<rdfs:subClassOf>
			<owl:Restriction>
				<owl:onProperty rdf:resource="&fibo-fnd-dt-fd;hasEndDate"/>
				<owl:onClass rdf:resource="&fibo-fnd-dt-fd;ExplicitDate"/>
				<owl:maxQualifiedCardinality rdf:datatype="&xsd;nonNegativeInteger">1</owl:maxQualifiedCardinality>
			</owl:Restriction>
		</rdfs:subClassOf>
		<rdfs:subClassOf>
			<owl:Restriction>
				<owl:onProperty rdf:resource="&fibo-fnd-dt-fd;hasStartDate"/>
				<owl:onClass rdf:resource="&fibo-fnd-dt-fd;ExplicitDate"/>
				<owl:maxQualifiedCardinality rdf:datatype="&xsd;nonNegativeInteger">1</owl:maxQualifiedCardinality>
			</owl:Restriction>
		</rdfs:subClassOf>
		<rdfs:subClassOf>
			<owl:Restriction>
				<owl:onProperty rdf:resource="&fibo-fnd-dt-fd;hasDuration"/>
				<owl:onClass rdf:resource="&fibo-fnd-dt-fd;ExplicitDuration"/>
				<owl:maxQualifiedCardinality rdf:datatype="&xsd;nonNegativeInteger">1</owl:maxQualifiedCardinality>
			</owl:Restriction>
		</rdfs:subClassOf>
		<rdfs:label>explicit date period</rdfs:label>
		<skos:definition>a date period for which the start date, end date, and duration are all explicit</skos:definition>
		<fibo-fnd-utl-av:usageNote>As with DatePeriod, any one of {start date, end date, duration} may be omitted because the missing property can be inferred from the other two.</fibo-fnd-utl-av:usageNote>
	</owl:Class>
	
	<owl:Class rdf:about="&fibo-fnd-dt-fd;ExplicitDuration">
		<rdfs:subClassOf rdf:resource="&fibo-fnd-dt-fd;Duration"/>
		<rdfs:subClassOf>
			<owl:Restriction>
				<owl:onProperty rdf:resource="&fibo-fnd-dt-fd;hasDurationValue"/>
				<owl:onDataRange rdf:resource="&xsd;string"/>
				<owl:qualifiedCardinality rdf:datatype="&xsd;nonNegativeInteger">1</owl:qualifiedCardinality>
			</owl:Restriction>
		</rdfs:subClassOf>
		<rdfs:label>explicit duration</rdfs:label>
		<skos:definition>a duration for which the &apos;hasDurationValue&apos; property must be set</skos:definition>
		<fibo-fnd-utl-av:explanatoryNote>This class is used when a duration is guaranteed to be known when it is created.</fibo-fnd-utl-av:explanatoryNote>
	</owl:Class>
	
	<owl:Class rdf:about="&fibo-fnd-dt-fd;ExplicitRecurrenceInterval">
		<rdfs:subClassOf rdf:resource="&fibo-fnd-dt-fd;RecurrenceInterval"/>
		<rdfs:subClassOf>
			<owl:Restriction>
				<owl:onProperty rdf:resource="&fibo-fnd-dt-fd;hasDurationValue"/>
				<owl:onDataRange rdf:resource="&xsd;string"/>
				<owl:qualifiedCardinality rdf:datatype="&xsd;nonNegativeInteger">1</owl:qualifiedCardinality>
			</owl:Restriction>
		</rdfs:subClassOf>
		<rdfs:label>explicit recurrence interval</rdfs:label>
		<skos:definition>a recurrence interval defined via an explicit duration</skos:definition>
	</owl:Class>
	
	<fibo-fnd-dt-fd:TimeInterval rdf:about="&fibo-fnd-dt-fd;Friday">
		<rdf:type rdf:resource="&owl;NamedIndividual"/>
		<rdfs:label>Friday</rdfs:label>
		<skos:definition>time interval that has duration 1 day and that meets a Saturday</skos:definition>
	</fibo-fnd-dt-fd:TimeInterval>
	
	<fibo-fnd-dt-fd:TimeDirection rdf:about="&fibo-fnd-dt-fd;FromEnd">
		<rdf:type rdf:resource="&owl;NamedIndividual"/>
		<rdfs:label>from the end</rdfs:label>
		<skos:definition>The CalendarSpecifiedDate is the nth date from the end of a calendar period.</skos:definition>
		<skos:example>Two days before the end of a calendar month.</skos:example>
	</fibo-fnd-dt-fd:TimeDirection>
	
	<fibo-fnd-dt-fd:TimeDirection rdf:about="&fibo-fnd-dt-fd;FromStart">
		<rdf:type rdf:resource="&owl;NamedIndividual"/>
		<rdfs:label>from the start</rdfs:label>
		<skos:definition>The CalendarSpecifiedDate is the nth day from the beginning of a calendar period.</skos:definition>
		<skos:example>The first day of a calendar quarter. (The offsetDay is zero.)</skos:example>
	</fibo-fnd-dt-fd:TimeDirection>
	
	<fibo-fnd-dt-fd:TimeInterval rdf:about="&fibo-fnd-dt-fd;Monday">
		<rdf:type rdf:resource="&owl;NamedIndividual"/>
		<rdfs:label>Monday</rdfs:label>
		<skos:definition>time interval that has duration 1 day and that meets a Tuesday</skos:definition>
	</fibo-fnd-dt-fd:TimeInterval>
	
	<owl:Class rdf:about="&fibo-fnd-dt-fd;RecurrenceInterval">
		<rdfs:subClassOf rdf:resource="&fibo-fnd-dt-fd;TimeInterval"/>
		<rdfs:label>recurrence interval</rdfs:label>
		<skos:definition>a time interval that is consistent between elements of a regular schedule</skos:definition>
		<fibo-fnd-utl-av:synonym>frequency</fibo-fnd-utl-av:synonym>
	</owl:Class>
	
	<owl:Class rdf:about="&fibo-fnd-dt-fd;RegularSchedule">
		<rdfs:subClassOf rdf:resource="&fibo-fnd-dt-fd;Schedule"/>
		<rdfs:subClassOf>
			<owl:Restriction>
				<owl:onProperty rdf:resource="&fibo-fnd-dt-fd;hasFinalStub"/>
				<owl:onClass rdf:resource="&fibo-fnd-dt-fd;ScheduleStub"/>
				<owl:maxQualifiedCardinality rdf:datatype="&xsd;nonNegativeInteger">1</owl:maxQualifiedCardinality>
			</owl:Restriction>
		</rdfs:subClassOf>
		<rdfs:subClassOf>
			<owl:Restriction>
				<owl:onProperty rdf:resource="&fibo-fnd-dt-fd;hasInitialStub"/>
				<owl:onClass rdf:resource="&fibo-fnd-dt-fd;ScheduleStub"/>
				<owl:maxQualifiedCardinality rdf:datatype="&xsd;nonNegativeInteger">1</owl:maxQualifiedCardinality>
			</owl:Restriction>
		</rdfs:subClassOf>
		<rdfs:subClassOf>
			<owl:Restriction>
				<owl:onProperty rdf:resource="&fibo-fnd-dt-fd;hasCount"/>
				<owl:maxQualifiedCardinality rdf:datatype="&xsd;nonNegativeInteger">1</owl:maxQualifiedCardinality>
				<owl:onDataRange rdf:resource="&xsd;positiveInteger"/>
			</owl:Restriction>
		</rdfs:subClassOf>
		<rdfs:subClassOf>
			<owl:Restriction>
				<owl:onProperty rdf:resource="&fibo-fnd-dt-fd;hasRecurrenceStartDate"/>
				<owl:onClass rdf:resource="&fibo-fnd-dt-fd;Date"/>
				<owl:qualifiedCardinality rdf:datatype="&xsd;nonNegativeInteger">1</owl:qualifiedCardinality>
			</owl:Restriction>
		</rdfs:subClassOf>
		<rdfs:subClassOf>
			<owl:Restriction>
				<owl:onProperty rdf:resource="&fibo-fnd-dt-fd;hasRecurrenceInterval"/>
				<owl:onClass rdf:resource="&fibo-fnd-dt-fd;RecurrenceInterval"/>
				<owl:qualifiedCardinality rdf:datatype="&xsd;nonNegativeInteger">1</owl:qualifiedCardinality>
			</owl:Restriction>
		</rdfs:subClassOf>
		<rdfs:label xml:lang="en">regular schedule</rdfs:label>
		<skos:definition>a schedule whose time intervals recur regularly</skos:definition>
		<skos:editorialNote>The BusinessDates ontology extends &apos;RegularSchedule&apos; with an optional BusinessDayAdjustment that specifies what should happen if a scheduled date falls on a weekend or a holiday.</skos:editorialNote>
		<skos:example>A 30 year mortgage is payable monthly on the 10th of the month, starting July 2015. The mortgage is issued on June 15, 2015 so the first payment is for the period June 15-June 30, and the last payment is for June 1-14 2045.

The payment schedule is a RegularSchedule with these properties:

* comprises: regular payment OccurrenceKind (with payment details)  (see the &apos;comprises&apos; property of the Occurrences ontology)
* hasInitialStub: June 15-30, 2015 for initial payment
* hasFinalStub: June 1-14, 2045 for final payment
* hasCount: 358
* hasOverallPeriod starting Date: June 15, 2015 with a duration of 30 years
* hasRecurrenceInterval: specifies 10th day of each calendar month
* hasRecurrenceStartDate: July 1, 2015</skos:example>
		<skos:example>A corporate bond pays interest for 10 years starting on the first day of 2015.  Interest payments are due 15 days after the expiration of each 6 month period: on July 15 and January 16.

The payment schedule is a RegularSchedule, with these properties:

* comprises: identifies the interest payment details
* overall DatePeriod starting date is &apos;2015-01-01&apos;, ending date is &apos;2025-01-15&apos;, and duration is &apos;P10Y15D&apos;
* hasCount is 20 (2 payments per year for 10 years)
* hasRecurrenceInterval is &apos;P6M&apos;
* hasRecurrenceStartDate is &apos;2015-01-15&apos;</skos:example>
		<fibo-fnd-utl-av:explanatoryNote>A RegularSchedule is a Schedule defined as a set of Dates that start on a recurrence start date and repeat after each recurrence interval.  The size of this set is defined by a count.

The &apos;initial ScheduleStub&apos; associated with a RegularSchedule identifies any special treatment applied before the recurrence start date.  Similarly, a &apos;final ScheduleStub&apos; identifies any special handling at the end of the recurrences.  For example, a mortgage loan that is due each calendar month may have an initial payment due before the first calendar month, or a final payment due after the last monthly payment.</fibo-fnd-utl-av:explanatoryNote>
		<fibo-fnd-utl-av:usageNote>Other ontologies can extend RegularSchedule as needed.

In particular, the Occurrences ontology extends RegularSchedule to &apos;comprise&apos; an &apos;OccurrenceKind&apos;.  The intended meaning is that a regular schedule comprises a number of scheduled dates and an event which is scheduled to occur on each of those dates, in other words an Occurrence of the OccurrenceKind should happen on each Date defined by the RegularSchedule.</fibo-fnd-utl-av:usageNote>
		<fibo-fnd-utl-av:usageNote>The recurrence start date can be an ExplicitDate or any kind of CalculatedDate.  Hence, the starting date could be relative to another Date (e.g. T+3) or triggered by the Occurrence of an OccurrenceKind, etc.

The recurrence start date can also be relative to the starting Date of the overall DatePeriod of the Schedule.</fibo-fnd-utl-av:usageNote>
	</owl:Class>
	
	<owl:Class rdf:about="&fibo-fnd-dt-fd;RelativeDate">
		<rdfs:subClassOf rdf:resource="&fibo-fnd-dt-fd;CalculatedDate"/>
		<rdfs:subClassOf>
			<owl:Restriction>
				<owl:onProperty rdf:resource="&fibo-fnd-dt-fd;isRelativeTo"/>
				<owl:onClass rdf:resource="&fibo-fnd-dt-fd;Date"/>
				<owl:qualifiedCardinality rdf:datatype="&xsd;nonNegativeInteger">1</owl:qualifiedCardinality>
			</owl:Restriction>
		</rdfs:subClassOf>
		<rdfs:subClassOf>
			<owl:Restriction>
				<owl:onProperty rdf:resource="&fibo-fnd-dt-fd;hasRelativeDuration"/>
				<owl:onDataRange rdf:resource="&xsd;string"/>
				<owl:qualifiedCardinality rdf:datatype="&xsd;nonNegativeInteger">1</owl:qualifiedCardinality>
			</owl:Restriction>
		</rdfs:subClassOf>
		<rdfs:label>relative date</rdfs:label>
		<owl:disjointWith rdf:resource="&fibo-fnd-dt-fd;SpecifiedDate"/>
		<skos:definition>a calculated date that is some duration before or after another date</skos:definition>
		<skos:example>A settlement date, defined as T+3: three days after the trade date.  The &apos;hasRelativeDuration&apos; property is set to &apos;3D&apos;.</skos:example>
		<fibo-fnd-utl-av:explanatoryNote>When the &apos;hasRelativeDuration&apos; property is negative, the RelativeDate is before the &apos;isRelativeTo&apos; Date; otherwise the RelativeDate is after the &apos;isRelativeTo&apos; Date.</fibo-fnd-utl-av:explanatoryNote>
	</owl:Class>
	
	<fibo-fnd-dt-fd:TimeInterval rdf:about="&fibo-fnd-dt-fd;Saturday">
		<rdf:type rdf:resource="&owl;NamedIndividual"/>
		<rdfs:label>Saturday</rdfs:label>
		<skos:definition>time interval that has duration 1 day and that meets a Sunday</skos:definition>
		<fibo-fnd-utl-av:explanatoryNote>One Saturday is the time interval that has duration 1 day and that starts Gregorian year 2000. This requirement anchors the repeating sequence of days of week to specific Gregorian days. It requires that January 1, 2000 is a Saturday. It follows that January 2, 2000 must be the Sunday that it meets, and so on.</fibo-fnd-utl-av:explanatoryNote>
	</fibo-fnd-dt-fd:TimeInterval>
	
	<owl:Class rdf:about="&fibo-fnd-dt-fd;Schedule">
		<rdfs:subClassOf rdf:resource="&fibo-fnd-arr-arr;Collection"/>
		<rdfs:subClassOf>
			<owl:Restriction>
				<owl:onProperty rdf:resource="&fibo-fnd-dt-fd;hasOverallPeriod"/>
				<owl:onClass rdf:resource="&fibo-fnd-dt-fd;DatePeriod"/>
				<owl:qualifiedCardinality rdf:datatype="&xsd;nonNegativeInteger">1</owl:qualifiedCardinality>
			</owl:Restriction>
		</rdfs:subClassOf>
		<rdfs:label>schedule</rdfs:label>
		<skos:definition>a collection of events or things that will be done and the dates and/or times when they will be done</skos:definition>
		<fibo-fnd-utl-av:adaptedFrom rdf:datatype="&xsd;anyURI">http://www.merriam-webster.com/dictionary/schedule</fibo-fnd-utl-av:adaptedFrom>
		<fibo-fnd-utl-av:explanatoryNote>The overall period covers the entire DatePeriod of the Schedule, from the earliest Date to the final Date of the Schedule. Schedules may be ad hoc, essentially a list of dates and events without any consistency in the durations between events, regular, in which case there is a consistently recurring interval between events, or a combination of the two.</fibo-fnd-utl-av:explanatoryNote>
	</owl:Class>
	
	<owl:Class rdf:about="&fibo-fnd-dt-fd;ScheduleStub">
		<rdfs:subClassOf rdf:resource="&fibo-fnd-arr-arr;Collection"/>
		<rdfs:subClassOf>
			<owl:Restriction>
				<owl:onProperty rdf:resource="&fibo-fnd-dt-fd;hasDatePeriod"/>
				<owl:onClass rdf:resource="&fibo-fnd-dt-fd;DatePeriod"/>
				<owl:qualifiedCardinality rdf:datatype="&xsd;nonNegativeInteger">1</owl:qualifiedCardinality>
			</owl:Restriction>
		</rdfs:subClassOf>
		<rdfs:label>schedule stub</rdfs:label>
		<skos:definition>a date period before the start of the recurring part of a schedule or after the end of the recurring part, which may be associated with a specific occurrence kind</skos:definition>
		<skos:editorialNote>The Occurrences ontology extends ScheduleStub to &apos;comprise&apos; an OccurrenceKind. The meaning is that a schedule stub comprises a date period and an event which is scheduled to occur during that date period; in other words that an Occurrence of the OccurrenceKind should happen during the DatePeriod of the ScheduleStub.</skos:editorialNote>
		<skos:example>A 30 year mortgage calls for monthly payments on the first day of each month, according to a RegularSchedule.  If the mortgage does not start on the first day of a calendar month, then an initial ScheduleStub specifies the payment due for the DatePeriod up to the first day of the next calendar month.  Similarly, a final ScheduleStub specifies the last payment due for the DatePeriod after the end of the last full calendar month.</skos:example>
	</owl:Class>
	
	<owl:Class rdf:about="&fibo-fnd-dt-fd;SpecifiedDate">
		<rdfs:subClassOf rdf:resource="&fibo-fnd-dt-fd;CalculatedDate"/>
		<rdfs:subClassOf>
			<owl:Restriction>
				<owl:onProperty rdf:resource="&fibo-fnd-dt-fd;hasDateSpecification"/>
				<owl:onDataRange rdf:resource="&xsd;string"/>
				<owl:qualifiedCardinality rdf:datatype="&xsd;nonNegativeInteger">1</owl:qualifiedCardinality>
			</owl:Restriction>
		</rdfs:subClassOf>
		<rdfs:label>specified date</rdfs:label>
		<skos:definition>a calculated date that is defined by a rule, which is captured as a string by the &apos;hasDateSpecification&apos; property</skos:definition>
	</owl:Class>
	
	<fibo-fnd-dt-fd:TimeInterval rdf:about="&fibo-fnd-dt-fd;Sunday">
		<rdf:type rdf:resource="&owl;NamedIndividual"/>
		<rdfs:label>Sunday</rdfs:label>
		<skos:definition>time interval that has duration 1 day and that meets a Monday</skos:definition>
	</fibo-fnd-dt-fd:TimeInterval>
	
	<fibo-fnd-dt-fd:TimeInterval rdf:about="&fibo-fnd-dt-fd;Thursday">
		<rdf:type rdf:resource="&owl;NamedIndividual"/>
		<rdfs:label>Thursday</rdfs:label>
		<skos:definition>time interval that has duration 1 day and that meets a Friday</skos:definition>
	</fibo-fnd-dt-fd:TimeInterval>
	
	<owl:Class rdf:about="&fibo-fnd-dt-fd;TimeDirection">
		<rdfs:label>time direction</rdfs:label>
		<skos:definition>an enumeration that indicates whether a calendar specified date is figured from the start or the end of a calendar period</skos:definition>
	</owl:Class>
	
	<owl:Class rdf:about="&fibo-fnd-dt-fd;TimeInterval">
		<rdfs:subClassOf rdf:resource="&fibo-fnd-plc-loc;Location"/>
		<rdfs:label>time interval</rdfs:label>
		<skos:definition>a segment of the time axis, a location in time</skos:definition>
		<skos:example>the day whose Gregorian calendar date is September 11, 2001</skos:example>
		<skos:example>the lifetime of Henry V</skos:example>
		<fibo-fnd-utl-av:adaptedFrom rdf:datatype="&xsd;anyURI">http://www.omg.org/spec/DTV/</fibo-fnd-utl-av:adaptedFrom>
		<fibo-fnd-utl-av:explanatoryNote>Every time interval has a beginning, an end, and a duration, even if not known. Every time interval is &apos;finite&apos;, a bounded segment of the time axis. The beginning or end of a time interval may be defined by reference to events that occur for a time interval that is not known.</fibo-fnd-utl-av:explanatoryNote>
		<fibo-fnd-utl-av:explanatoryNote>Time intervals may be indefinite, meaning that their beginning is primordiality or their end is perpetuity, or both (eternity). This vocabulary assumes that indefinite time intervals exist and have some duration, but their duration is unknown.</fibo-fnd-utl-av:explanatoryNote>
	</owl:Class>
	
	<fibo-fnd-dt-fd:TimeInterval rdf:about="&fibo-fnd-dt-fd;Tuesday">
		<rdf:type rdf:resource="&owl;NamedIndividual"/>
		<rdfs:label>Tuesday</rdfs:label>
		<skos:definition>time interval that has duration 1 day and that meets a Wednesday</skos:definition>
	</fibo-fnd-dt-fd:TimeInterval>
	
	<fibo-fnd-dt-fd:TimeInterval rdf:about="&fibo-fnd-dt-fd;Wednesday">
		<rdf:type rdf:resource="&owl;NamedIndividual"/>
		<rdfs:label>Wednesday</rdfs:label>
		<skos:definition>time interval that has duration 1 day and that meets a Thursday</skos:definition>
	</fibo-fnd-dt-fd:TimeInterval>
	
	<rdfs:Datatype rdf:about="&fibo-fnd-dt-fd;dateValue">
		<rdfs:label>date value</rdfs:label>
		<owl:deprecated rdf:datatype="&xsd;boolean">true</owl:deprecated>
		<owl:equivalentClass rdf:resource="&xsd;string"/>
		<skos:definition>a literal (explicit) date captured in the format specified for xsd:date (i.e., ISO 8601 format), WITHOUT a timezone field; the semantics are identical to those of xsd:date</skos:definition>
		<skos:editorialNote>This datatype substitutes for xsd:date, which OWL 2 does not support.</skos:editorialNote>
		<skos:example>2002-10-10 means October 10, 2002</skos:example>
		<fibo-fnd-utl-av:usageNote>For consistency with FPML (reference FPML Coding Schemes 30 June 2014, Version 1.56, section 2.1.1), the year MUST be specified as 4 digits, and the month and day MUST be specified as 2 digits with a leading zero if needed. Times and timezones should NOT be specified.</fibo-fnd-utl-av:usageNote>
	</rdfs:Datatype>
	
	<rdfs:Datatype rdf:about="&fibo-fnd-dt-fd;durationValue">
		<rdfs:label>duration value</rdfs:label>
		<owl:deprecated rdf:datatype="&xsd;boolean">true</owl:deprecated>
		<owl:equivalentClass rdf:resource="&xsd;string"/>
		<skos:definition>a literal (explicit) duration (amount of time) captured in the format specified for xsd:duration (i.e., ISO 8601 format); the semantics are identical to those of xsd:duration</skos:definition>
		<skos:editorialNote>This datatype substitutes for xsd:duration, which OWL2 does not support.</skos:editorialNote>
		<skos:example>-P3D means negative 3 days duration. This is used with OffsetDates to specify 3 days before (prior) to some other Date.</skos:example>
		<skos:example>P1Y means 1 year</skos:example>
		<skos:example>P1Y2M3DT4H5M6S means 1 year, 2 months, 3 days, 4 hours, 5 minutes, 6 seconds</skos:example>
		<skos:example>P2M means 2 months</skos:example>
		<skos:example>P3D means 3 days</skos:example>
		<skos:example>PT4H means 4 hours</skos:example>
		<skos:example>PT5M means 5 minutes</skos:example>
		<skos:example>PT6S means 6 seconds</skos:example>
		<fibo-fnd-utl-av:usageNote>Negative durations are used to indicate relative dates that are before (rather than after) some other Date.</fibo-fnd-utl-av:usageNote>
	</rdfs:Datatype>
	
	<owl:ObjectProperty rdf:about="&fibo-fnd-dt-fd;hasAsOfDate">
		<rdfs:subPropertyOf rdf:resource="&fibo-fnd-dt-fd;hasDate"/>
		<rdfs:label>as of date</rdfs:label>
		<skos:definition>relates something to the date on which it is accurate or valid (e.g. a credit report has an asOfDate that means the date when the information was drawn)</skos:definition>
		<fibo-fnd-utl-av:explanatoryNote>It is different from the creation date and need not be the last date of the DatePeriod covered.</fibo-fnd-utl-av:explanatoryNote>
	</owl:ObjectProperty>
	
	<owl:ObjectProperty rdf:about="&fibo-fnd-dt-fd;hasCalendarPeriod">
		<rdfs:subPropertyOf rdf:resource="&fibo-fnd-rel-rel;has"/>
		<rdfs:label>has calendar period</rdfs:label>
		<rdfs:range rdf:resource="&fibo-fnd-dt-fd;CalendarPeriod"/>
		<skos:definition>identifies a calendar period used in computing a CalendarSpecifiedDate, such as a calendar week, calendar month, calendar quarter, or calendar year</skos:definition>
	</owl:ObjectProperty>
	
	<owl:DatatypeProperty rdf:about="&fibo-fnd-dt-fd;hasCount">
		<rdfs:label>has count</rdfs:label>
		<rdfs:range rdf:resource="&xsd;positiveInteger"/>
		<skos:definition>indicates the number of things in a collection, such as the number of entries in a RegularSchedule</skos:definition>
	</owl:DatatypeProperty>
	
	<owl:ObjectProperty rdf:about="&fibo-fnd-dt-fd;hasDate">
		<rdfs:subPropertyOf rdf:resource="&fibo-fnd-rel-rel;has"/>
		<rdfs:label>has date</rdfs:label>
		<rdfs:range rdf:resource="&fibo-fnd-dt-fd;Date"/>
		<skos:definition>identifies a specific date</skos:definition>
	</owl:ObjectProperty>
	
	<owl:ObjectProperty rdf:about="&fibo-fnd-dt-fd;hasDatePeriod">
		<rdfs:subPropertyOf rdf:resource="&fibo-fnd-rel-rel;has"/>
		<rdfs:label>has date period</rdfs:label>
		<rdfs:range rdf:resource="&fibo-fnd-dt-fd;DatePeriod"/>
		<skos:definition>identifies a specific period of time, including a start date, end date and or duration</skos:definition>
	</owl:ObjectProperty>
	
	<owl:ObjectProperty rdf:about="&fibo-fnd-dt-fd;hasDateReceived">
		<rdfs:subPropertyOf rdf:resource="&fibo-fnd-dt-fd;hasDate"/>
		<rdfs:label>has date received</rdfs:label>
		<skos:definition>relates something to the date when it was received, e.g. a loan application request</skos:definition>
	</owl:ObjectProperty>
	
	<owl:DatatypeProperty rdf:about="&fibo-fnd-dt-fd;hasDateSpecification">
		<rdfs:label>has date specification</rdfs:label>
		<rdfs:domain rdf:resource="&fibo-fnd-dt-fd;SpecifiedDate"/>
		<rdfs:range rdf:resource="&xsd;string"/>
		<skos:definition>A rule that specifies how a SpecifiedDate is computed.</skos:definition>
		<skos:editorialNote>The rule is modeled as a simple String because OWL2 provides no way to model the semantics of such a rule.</skos:editorialNote>
	</owl:DatatypeProperty>
	
	<owl:ObjectProperty rdf:about="&fibo-fnd-dt-fd;hasDateTime">
		<rdfs:subPropertyOf rdf:resource="&fibo-fnd-rel-rel;has"/>
		<rdfs:label>has date time</rdfs:label>
		<rdfs:range rdf:resource="&fibo-fnd-dt-fd;DateTime"/>
		<skos:definition>identifies a specific date and time of day, excluding the time zone</skos:definition>
	</owl:ObjectProperty>
	
	<owl:ObjectProperty rdf:about="&fibo-fnd-dt-fd;hasDateTimeStamp">
		<rdfs:subPropertyOf rdf:resource="&fibo-fnd-rel-rel;has"/>
		<rdfs:label>has date time stamp</rdfs:label>
		<rdfs:range rdf:resource="&fibo-fnd-dt-fd;DateTimeStamp"/>
		<skos:definition>identifies a specific date and time of day, including the time zone</skos:definition>
	</owl:ObjectProperty>
	
	<owl:DatatypeProperty rdf:about="&fibo-fnd-dt-fd;hasDateTimeStampValue">
		<rdfs:label>has date time stamp value</rdfs:label>
		<rdfs:range rdf:resource="&xsd;dateTimeStamp"/>
		<skos:definition>specifies an actual literal (explicit) date and time, including the time zone</skos:definition>
	</owl:DatatypeProperty>
	
	<owl:DatatypeProperty rdf:about="&fibo-fnd-dt-fd;hasDateTimeValue">
		<rdfs:label>has date time value</rdfs:label>
		<rdfs:range rdf:resource="&xsd;dateTime"/>
		<skos:definition>specifies an actual literal (explicit) date and time</skos:definition>
	</owl:DatatypeProperty>
	
	<owl:DatatypeProperty rdf:about="&fibo-fnd-dt-fd;hasDateValue">
		<rdfs:label>has date value</rdfs:label>
		<rdfs:range rdf:resource="&xsd;string"/>
		<skos:definition>specifies an actual literal (explicit) date captured in the format specified for xsd:date (i.e., ISO 8601 format), WITHOUT the time or timezone information; the semantics are identical to those of xsd:date</skos:definition>
		<skos:example>2002-10-10 means October 10, 2002</skos:example>
		<fibo-fnd-utl-av:usageNote>For consistency with FPML (reference FPML Coding Schemes 30 June 2014, Version 1.56, section 2.1.1), the year MUST be specified as 4 digits, and the month and day MUST be specified as 2 digits with a leading zero if needed. Times and timezones should NOT be specified.</fibo-fnd-utl-av:usageNote>
	</owl:DatatypeProperty>
	
	<rdf:Description rdf:about="&fibo-fnd-dt-fd;hasDuration">
		<rdf:type rdf:resource="&owl;FunctionalProperty"/>
		<rdf:type rdf:resource="&owl;ObjectProperty"/>
		<rdfs:subPropertyOf rdf:resource="&fibo-fnd-rel-rel;has"/>
		<rdfs:label>has duration</rdfs:label>
		<rdfs:range rdf:resource="&fibo-fnd-dt-fd;Duration"/>
		<skos:definition>the duration of a date period or similar concept, such as the tenor of a contract</skos:definition>
		<fibo-fnd-utl-av:usageNote>This duration may be omitted or unknown if either the start or end Date of the DatePeriod is a CalculatedDate or an ExplicitDate.</fibo-fnd-utl-av:usageNote>
	</rdf:Description>
	
	<owl:DatatypeProperty rdf:about="&fibo-fnd-dt-fd;hasDurationValue">
		<rdfs:label>has duration value</rdfs:label>
		<rdfs:domain rdf:resource="&fibo-fnd-dt-fd;Duration"/>
		<rdfs:range rdf:resource="&xsd;string"/>
		<skos:definition>specifies a literal (explicit) duration (amount of time) captured in the format specified for xsd:duration (i.e., ISO 8601 format); the semantics are identical to those of xsd:duration</skos:definition>
		<skos:example>-P3D means negative 3 days duration. This is used with OffsetDates to specify 3 days before (prior) to some other Date.</skos:example>
		<skos:example>P1Y means 1 year</skos:example>
		<skos:example>P1Y2M3DT4H5M6S means 1 year, 2 months, 3 days, 4 hours, 5 minutes, 6 seconds</skos:example>
		<skos:example>P2M means 2 months</skos:example>
		<skos:example>P3D means 3 days</skos:example>
		<skos:example>PT4H means 4 hours</skos:example>
		<skos:example>PT5M means 5 minutes</skos:example>
		<skos:example>PT6S means 6 seconds</skos:example>
		<fibo-fnd-utl-av:usageNote>Negative durations are used to indicate relative dates that are before (rather than after) some other Date.</fibo-fnd-utl-av:usageNote>
	</owl:DatatypeProperty>
	
	<rdf:Description rdf:about="&fibo-fnd-dt-fd;hasEndDate">
		<rdf:type rdf:resource="&owl;FunctionalProperty"/>
		<rdf:type rdf:resource="&owl;ObjectProperty"/>
		<rdfs:subPropertyOf rdf:resource="&fibo-fnd-dt-fd;hasDate"/>
		<rdfs:label>has end date</rdfs:label>
		<skos:definition>the ending date of some Schedule or DatePeriod</skos:definition>
	</rdf:Description>
	
	<rdf:Description rdf:about="&fibo-fnd-dt-fd;hasExplicitDate">
		<rdf:type rdf:resource="&owl;FunctionalProperty"/>
		<rdf:type rdf:resource="&owl;ObjectProperty"/>
		<rdfs:subPropertyOf rdf:resource="&fibo-fnd-dt-fd;hasDate"/>
		<rdfs:label>has explicit date</rdfs:label>
		<rdfs:range rdf:resource="&fibo-fnd-dt-fd;ExplicitDate"/>
	</rdf:Description>
	
	<owl:ObjectProperty rdf:about="&fibo-fnd-dt-fd;hasFinalStub">
		<rdfs:subPropertyOf rdf:resource="&fibo-fnd-dt-fd;hasStub"/>
		<rdfs:label>has final stub</rdfs:label>
		<skos:definition>identifies any special period at the end of a regular schedule</skos:definition>
	</owl:ObjectProperty>
	
	<owl:ObjectProperty rdf:about="&fibo-fnd-dt-fd;hasInitialStub">
		<rdfs:subPropertyOf rdf:resource="&fibo-fnd-dt-fd;hasStub"/>
		<rdfs:label>has initial stub</rdfs:label>
		<skos:definition>identifies any special period at the start of a regular schedule</skos:definition>
	</owl:ObjectProperty>
	
	<owl:DatatypeProperty rdf:about="&fibo-fnd-dt-fd;hasOrdinalNumber">
		<rdfs:label>has ordinal number</rdfs:label>
		<rdfs:range rdf:resource="&xsd;integer"/>
		<skos:definition>An ordinal number meaning 1st, 2nd, 3rd, etc.</skos:definition>
		<fibo-fnd-utl-av:explanatoryNote>Negative ordinal numbers mean 1st before, 2nd before, etc.</fibo-fnd-utl-av:explanatoryNote>
	</owl:DatatypeProperty>
	
	<owl:ObjectProperty rdf:about="&fibo-fnd-dt-fd;hasOverallPeriod">
		<rdfs:subPropertyOf rdf:resource="&fibo-fnd-dt-fd;hasDatePeriod"/>
		<rdfs:label>has overall period</rdfs:label>
		<rdfs:domain rdf:resource="&fibo-fnd-dt-fd;Schedule"/>
		<skos:definition>identifies a DatePeriod that includes all the Dates of a Schedule, including any ScheduleStubs</skos:definition>
	</owl:ObjectProperty>
	
	<owl:ObjectProperty rdf:about="&fibo-fnd-dt-fd;hasRecurrenceInterval">
		<rdfs:subPropertyOf rdf:resource="&fibo-fnd-rel-rel;has"/>
		<rdfs:label>has recurrence interval</rdfs:label>
		<rdfs:range rdf:resource="&fibo-fnd-dt-fd;RecurrenceInterval"/>
	</owl:ObjectProperty>
	
	<owl:ObjectProperty rdf:about="&fibo-fnd-dt-fd;hasRecurrenceStartDate">
		<rdfs:subPropertyOf rdf:resource="&fibo-fnd-dt-fd;hasStartDate"/>
		<rdfs:label>has recurrence start date</rdfs:label>
		<skos:definition>the starting Date of the first recurrence of a RegularSchedule</skos:definition>
	</owl:ObjectProperty>
	
	<owl:DatatypeProperty rdf:about="&fibo-fnd-dt-fd;hasRelativeDuration">
		<rdfs:label>has relative duration</rdfs:label>
		<rdfs:range rdf:resource="&xsd;string"/>
		<skos:definition>a duration between two explicit dates</skos:definition>
		<fibo-fnd-utl-av:explanatoryNote>A relative duration may be negative.</fibo-fnd-utl-av:explanatoryNote>
		<fibo-fnd-utl-av:explanatoryNote>Note that this property is distinct from hasDurationValue, as a relative duration may resolve to a relative date or date time (both of which are time points) rather than an interval, which would result in a logical inconsistency if its parent property is hasDurationValue.</fibo-fnd-utl-av:explanatoryNote>
	</owl:DatatypeProperty>
	
	<owl:ObjectProperty rdf:about="&fibo-fnd-dt-fd;hasSchedule">
		<rdfs:subPropertyOf rdf:resource="&fibo-fnd-rel-rel;has"/>
		<rdfs:label>has schedule</rdfs:label>
		<rdfs:range rdf:resource="&fibo-fnd-dt-fd;Schedule"/>
		<skos:definition>indicates a schedule for something</skos:definition>
	</owl:ObjectProperty>
	
	<rdf:Description rdf:about="&fibo-fnd-dt-fd;hasStartDate">
		<rdf:type rdf:resource="&owl;FunctionalProperty"/>
		<rdf:type rdf:resource="&owl;ObjectProperty"/>
		<rdfs:subPropertyOf rdf:resource="&fibo-fnd-dt-fd;hasDate"/>
		<rdfs:label>has start date</rdfs:label>
		<skos:definition>the starting Date of something</skos:definition>
	</rdf:Description>
	
	<owl:ObjectProperty rdf:about="&fibo-fnd-dt-fd;hasStub">
		<rdfs:subPropertyOf rdf:resource="&fibo-fnd-rel-rel;has"/>
		<rdfs:label>has stub</rdfs:label>
		<rdfs:domain rdf:resource="&fibo-fnd-dt-fd;RegularSchedule"/>
		<rdfs:range rdf:resource="&fibo-fnd-dt-fd;ScheduleStub"/>
	</owl:ObjectProperty>
	
	<owl:ObjectProperty rdf:about="&fibo-fnd-dt-fd;hasTimeDirection">
		<rdfs:subPropertyOf rdf:resource="&fibo-fnd-rel-rel;has"/>
		<rdfs:label>has time direction</rdfs:label>
		<rdfs:range rdf:resource="&fibo-fnd-dt-fd;TimeDirection"/>
		<skos:definition>A TimeDirection indicates whether a CalendarSpecifiedDate is figured from the beginning or end of a calendar period.</skos:definition>
	</owl:ObjectProperty>
	
	<owl:ObjectProperty rdf:about="&fibo-fnd-dt-fd;isRelativeTo">
		<rdfs:label>is relative to</rdfs:label>
		<rdfs:range rdf:resource="&fibo-fnd-dt-fd;Date"/>
		<skos:definition>identifies a RelativeDate or RelativeDatePeriod defined relative to this Date</skos:definition>
	</owl:ObjectProperty>

</rdf:RDF>