<?xml version="1.0" encoding="UTF-8"?>
<rdf:RDF xmlns:xsd="http://www.w3.org/2001/XMLSchema#"
         xmlns:sm="http://www.omg.org/techprocess/ab/SpecificationMetadata/"
         xmlns:fibo-fnd-utl-av="http://www.omg.org/spec/EDMC-FIBO/FND/Utilities/AnnotationVocabulary/"
         xmlns:rdf="http://www.w3.org/1999/02/22-rdf-syntax-ns#"
         xmlns:rdfs="http://www.w3.org/2000/01/rdf-schema#"
         xmlns:owl="http://www.w3.org/2002/07/owl#"
         xmlns:skos="http://www.w3.org/2004/02/skos/core#"
         xmlns:dc="http://purl.org/dc/terms/"
         xml:base="http://www.omg.org/spec/EDMC-FIBO/pre-IND/Indicators/IndicatorsParameters/">

   <owl:Ontology rdf:about="http://www.omg.org/spec/EDMC-FIBO/pre-IND/Indicators/IndicatorsParameters/"/>

   <!--Datatypes-->

<!--Object Properties-->

<owl:ObjectProperty rdf:about="http://www.omg.org/spec/EDMC-FIBO/pre-IND/Indicators/IndicatorsParameters/financialInformationPublisherHasIdentity">
      <rdfs:subPropertyOf rdf:resource="http://www.edmcouncil.org/spec/EDMC-SR/FND/Publications/Publications/publisherIdentity"/>
      <rdfs:domain rdf:resource="http://www.omg.org/spec/EDMC-FIBO/pre-IND/Indicators/IndicatorsParameters/FinancialInformationPublisher"/>
      <rdfs:range rdf:resource="http://www.omg.org/spec/EDMC-SR/BE/LegalEntities/FormalBusinessOrganizations/FormallyConstitutedOrganization"/>
   </owl:ObjectProperty>

   <owl:ObjectProperty rdf:about="http://www.omg.org/spec/EDMC-FIBO/pre-IND/Indicators/IndicatorsParameters/marketSpreadIsBetween">
      <rdfs:subPropertyOf rdf:resource="http://www.omg.org/spec/EDMC-FIBO/MD/TemporalCore/InstrumentTemporalTerms/spreadIsBetween"/>
      <rdfs:subPropertyOf rdf:resource="http://www.omg.org/spec/FIBO/BE/Math/"/>
      <rdfs:domain rdf:resource="http://www.omg.org/spec/EDMC-FIBO/pre-IND/Indicators/IndicatorsParameters/MarketSpread"/>
      <rdfs:range rdf:resource="http://www.omg.org/spec/EDMC-FIBO/pre-IND/Indicators/IndicatorsParameters/MarketReferentialParameter"/>
   </owl:ObjectProperty>

   <owl:ObjectProperty rdf:about="http://www.omg.org/spec/EDMC-FIBO/pre-IND/Indicators/IndicatorsParameters/isVolatilityOf">
      <skos:definition>The market rate to which the volatility measure applies and of which it is a measure.</skos:definition>
      <rdfs:subPropertyOf rdf:resource="http://www.omg.org/spec/EDMC-SR/FND/Relations/Relations/appliesTo"/>
      <rdfs:subPropertyOf rdf:resource="http://www.edmcouncil.org/spec/EDMC-SR/FND/Math/Math/parameterAppliesTo"/>
      <rdfs:domain rdf:resource="http://www.omg.org/spec/EDMC-FIBO/pre-IND/Indicators/IndicatorsParameters/Volatility"/>
      <rdfs:range rdf:resource="http://www.omg.org/spec/EDMC-FIBO/pre-IND/Indicators/IndicatorsParameters/MarketBaseRate"/>
   </owl:ObjectProperty>

   <owl:ObjectProperty rdf:about="http://www.omg.org/spec/EDMC-FIBO/pre-IND/Indicators/IndicatorsParameters/isPublishedBy">
      <rdfs:subPropertyOf rdf:resource="http://www.edmcouncil.org/spec/EDMC-SR/FND/Publications/Publications/publishedBy"/>
      <rdfs:subPropertyOf rdf:resource="http://www.omg.org/spec/EDMC-SR/FND/Relations/Relations/isProvidedBy"/>
      <rdfs:domain rdf:resource="http://www.omg.org/spec/EDMC-FIBO/pre-IND/Indicators/IndicatorsParameters/MarketReferentialParameter"/>
      <rdfs:range rdf:resource="http://www.omg.org/spec/EDMC-FIBO/pre-IND/Indicators/IndicatorsParameters/FinancialInformationPublisher"/>
      <owl:inverseOf rdf:resource="http://www.omg.org/spec/EDMC-FIBO/pre-IND/Indicators/IndicatorsParameters/publishes"/>
   </owl:ObjectProperty>

   <owl:ObjectProperty rdf:about="http://www.omg.org/spec/EDMC-FIBO/pre-IND/Indicators/IndicatorsParameters/publishes">
      <skos:definition>Information published by the publisher, in the form of some market referential parameter such as an economic index or indicator.</skos:definition>
      <rdfs:subPropertyOf rdf:resource="http://www.omg.org/spec/EDMC-SR/FND/Relations/Relations/provides"/>
      <rdfs:domain rdf:resource="http://www.omg.org/spec/EDMC-FIBO/pre-IND/Indicators/IndicatorsParameters/FinancialInformationPublisher"/>
      <rdfs:range rdf:resource="http://www.omg.org/spec/EDMC-FIBO/pre-IND/Indicators/IndicatorsParameters/MarketReferentialParameter"/>
   </owl:ObjectProperty>

   <!--Data Properties-->

<!--Annotation Properties-->

<!--Classes-->

<owl:Class rdf:about="http://www.omg.org/spec/EDMC-FIBO/pre-IND/Indicators/IndicatorsParameters/FinancialInformationPublisher">
      <rdfs:label>Financial Information Publisher</rdfs:label>
      <skos:definition>Some entity which is acting in the capacity of a publisher or provider of information relating to the financial markets, or information which is of interest to those markets including information on economies, governments etc.</skos:definition>
      <rdfs:subClassOf rdf:resource="http://www.edmcouncil.org/spec/EDMC-SR/FND/Publications/Publications/Publisher"/>
   </owl:Class>

   <owl:Class rdf:about="http://www.omg.org/spec/EDMC-FIBO/pre-IND/Indicators/IndicatorsParameters/MarketBaseRate">
      <rdfs:label>Market Base Rate</rdfs:label>
      <skos:definition>Calculated notional value used to measure market trends for a set of instruments (S&amp;amp;P500, NASDAQ composite, 30day CD) or express economical climate for an industry (DowJones Industrial, H&amp;amp;Q Growth Technologies) and/or political region (Libor, Prime)</skos:definition>
      <skos:editorialNote>These are the types of Market Base, as established by an earlier industry expert review: Index: Statistical composite that measures changes in the economy or in financial markets, often expressed in percentage changes from a base year or from the previous month. source1 Money Rate: Benchmark or guideline for interest rates determined by central banks or economical climate as a whole Banker's Acceptance Rate: Benchmark reflecting market fluctuations of Bankerâ€™s Acceptance issued instruments. Commercial Paper Rate: Benchmark reflecting market fluctuations of Commercial Paper issued instruments. Certificate of Deposit Rate: Benchmark reflecting market fluctuations of Certificate of Deposit issued instruments. Interbank Rate Prime Time Deposit Rate: Benchmark reflecting market fluctuations of Deposit/Redeposit issued instruments. NOTE: The above definition was achieved by a large number of financial experts working together on this matter. This was over 16 years ago so no reference. Included instutitions such as JPM, Euroclear, Citi. General description: Calculated notional value used to measure market trends for a set of instruments. Includes regions, economies, and so on. Hence sub sets for different types of market bases.</skos:editorialNote>
      <rdfs:subClassOf rdf:resource="http://www.omg.org/spec/EDMC-FIBO/pre-IND/Indicators/IndicatorsParameters/MarketReferentialParameter"/>
   </owl:Class>

   <owl:Class rdf:about="http://www.omg.org/spec/EDMC-FIBO/pre-IND/Indicators/IndicatorsParameters/MarketReferentialParameter">
      <rdfs:label>Market Referential Parameter</rdfs:label>
      <skos:definition>A published parameter about financial or other markets, such as an index, an indicator or an interest rate.</skos:definition>
      <skos:editorialNote>Known collectively (in the CFI Standard) as Referential Instruments.</skos:editorialNote>
      <rdfs:subClassOf rdf:resource="http://www.edmcouncil.org/spec/EDMC-SR/FND/Math/Math/TimedParameter"/>
      <rdfs:subClassOf rdf:resource="http://www.omg.org/spec/EDMC-FIBO/MD/TemporalCore/InstrumentTemporalTerms/FinancialMarketInformation"/>
   </owl:Class>

   <owl:Class rdf:about="http://www.omg.org/spec/EDMC-FIBO/pre-IND/Indicators/IndicatorsParameters/MarketSpread">
      <rdfs:label>Market Spread</rdfs:label>
      <skos:definition>A published spread between some two market rates.</skos:definition>
      <rdfs:subClassOf rdf:resource="http://www.omg.org/spec/EDMC-FIBO/MD/TemporalCore/InstrumentTemporalTerms/Spread"/>
   </owl:Class>

   <owl:Class rdf:about="http://www.omg.org/spec/EDMC-FIBO/pre-IND/Indicators/IndicatorsParameters/Volatility">
      <rdfs:label>Volatility</rdfs:label>
      <skos:definition>A measure of security price fluctuation. Mathematically the volatility is the annualized standard deviation of a security's daily price changes</skos:definition>
   </owl:Class>

   <!--Individuals-->

</rdf:RDF>