<?xml version="1.0" encoding="UTF-8"?>
<!DOCTYPE rdf:RDF [
	<!ENTITY fibo-fnd-dt-fd "https://spec.edmcouncil.org/fibo/FND/DatesAndTimes/FinancialDates/">
	<!ENTITY fibo-fnd-math-math "https://spec.edmcouncil.org/fibo/FND/MathExt/Math/">
	<!ENTITY fibo-fnd-tim-tim "https://spec.edmcouncil.org/fibo/FND/TimeExt/Time/">
	<!ENTITY fibo-fnd-utl-av "https://spec.edmcouncil.org/fibo/FND/Utilities/AnnotationVocabulary/">
	<!ENTITY fibo-fnd-utlx-val "https://spec.edmcouncil.org/fibo/FND/UtilitiesExt/Values/">
	<!ENTITY fibo-ind-indx-valx "https://spec.edmcouncil.org/fibo/IND/IndicatorsExt/IndicatorsValues/">
	<!ENTITY fibo-md-temx-tem "https://spec.edmcouncil.org/fibo/MD/TemporalCore/TemporalConcepts/">
	<!ENTITY owl "http://www.w3.org/2002/07/owl#">
	<!ENTITY rdf "http://www.w3.org/1999/02/22-rdf-syntax-ns#">
	<!ENTITY rdfs "http://www.w3.org/2000/01/rdf-schema#">
	<!ENTITY skos "http://www.w3.org/2004/02/skos/core#">
	<!ENTITY xsd "http://www.w3.org/2001/XMLSchema#">
]>
<rdf:RDF xml:base="https://spec.edmcouncil.org/fibo/IND/IndicatorsExt/IndicatorsValues/"
	xmlns:fibo-fnd-dt-fd="https://spec.edmcouncil.org/fibo/FND/DatesAndTimes/FinancialDates/"
	xmlns:fibo-fnd-math-math="https://spec.edmcouncil.org/fibo/FND/MathExt/Math/"
	xmlns:fibo-fnd-tim-tim="https://spec.edmcouncil.org/fibo/FND/TimeExt/Time/"
	xmlns:fibo-fnd-utl-av="https://spec.edmcouncil.org/fibo/FND/Utilities/AnnotationVocabulary/"
	xmlns:fibo-fnd-utlx-val="https://spec.edmcouncil.org/fibo/FND/UtilitiesExt/Values/"
	xmlns:fibo-ind-indx-valx="https://spec.edmcouncil.org/fibo/IND/IndicatorsExt/IndicatorsValues/"
	xmlns:fibo-md-temx-tem="https://spec.edmcouncil.org/fibo/MD/TemporalCore/TemporalConcepts/"
	xmlns:owl="http://www.w3.org/2002/07/owl#"
	xmlns:rdf="http://www.w3.org/1999/02/22-rdf-syntax-ns#"
	xmlns:rdfs="http://www.w3.org/2000/01/rdf-schema#"
	xmlns:skos="http://www.w3.org/2004/02/skos/core#"
	xmlns:xsd="http://www.w3.org/2001/XMLSchema#">
	
	<owl:Ontology rdf:about="https://spec.edmcouncil.org/fibo/IND/IndicatorsExt/IndicatorsValues/">
		<rdfs:label xml:lang="en">IndicatorsValues</rdfs:label>
		<owl:imports rdf:resource="http://www.w3.org/2004/02/skos/core"/>
		<owl:imports rdf:resource="https://spec.edmcouncil.org/fibo/FND/DatesAndTimes/FinancialDates/"/>
		<owl:imports rdf:resource="https://spec.edmcouncil.org/fibo/FND/MathExt/Math/"/>
		<owl:imports rdf:resource="https://spec.edmcouncil.org/fibo/FND/TimeExt/Time/"/>
		<owl:imports rdf:resource="https://spec.edmcouncil.org/fibo/FND/Utilities/AnnotationVocabulary/"/>
		<owl:imports rdf:resource="https://spec.edmcouncil.org/fibo/FND/UtilitiesExt/Values/"/>
		<owl:imports rdf:resource="https://spec.edmcouncil.org/fibo/MD/TemporalCore/TemporalConcepts/"/>
		<owl:versionIRI rdf:resource="https://spec.edmcouncil.org/fibo/IND/IndicatorsExt/IndicatorsValues/"/>
		<fibo-fnd-utl-av:hasMaturityLevel rdf:resource="&fibo-fnd-utl-av;Informative"/>
	</owl:Ontology>
	
	<owl:Class rdf:about="&fibo-ind-indx-valx;EconomicRateQualifiedTimedValue">
		<rdfs:subClassOf rdf:resource="&fibo-ind-indx-valx;MarketParameterTimedValue"/>
		<rdfs:label xml:lang="en">economic rate qualified timed value  (please review)</rdfs:label>
		<owl:disjointWith rdf:resource="&fibo-ind-indx-valx;ExchangeRateTimedValue"/>
		<owl:disjointWith rdf:resource="&fibo-ind-indx-valx;InterestRateTimedValue"/>
		<owl:disjointWith rdf:resource="&fibo-ind-indx-valx;ReferenceIndexDatedValue"/>
	</owl:Class>
	
	<owl:Class rdf:about="&fibo-ind-indx-valx;ExchangeRateTimedValue">
		<rdfs:subClassOf rdf:resource="&fibo-ind-indx-valx;MarketParameterTimedValue"/>
		<rdfs:label xml:lang="en">exchange rate timed value  (please review)</rdfs:label>
		<owl:disjointWith rdf:resource="&fibo-ind-indx-valx;InterestRateTimedValue"/>
		<owl:disjointWith rdf:resource="&fibo-ind-indx-valx;ReferenceIndexDatedValue"/>
	</owl:Class>
	
	<owl:Class rdf:about="&fibo-ind-indx-valx;GDPValue">
		<rdfs:subClassOf rdf:resource="&fibo-ind-indx-valx;EconomicRateQualifiedTimedValue"/>
		<rdfs:label xml:lang="en">g d p value  (please review)</rdfs:label>
		<owl:disjointWith rdf:resource="&fibo-ind-indx-valx;InflationRateValue"/>
		<owl:disjointWith rdf:resource="&fibo-ind-indx-valx;UnemploymentRateValue"/>
	</owl:Class>
	
	<owl:Class rdf:about="&fibo-ind-indx-valx;InflationRateValue">
		<rdfs:subClassOf rdf:resource="&fibo-ind-indx-valx;EconomicRateQualifiedTimedValue"/>
		<rdfs:label xml:lang="en">inflation rate value  (please review)</rdfs:label>
		<owl:disjointWith rdf:resource="&fibo-ind-indx-valx;UnemploymentRateValue"/>
		<skos:definition xml:lang="en">The inflation rate, as a percentage. This is quoted for a period of time leading up to a specific date or month.</skos:definition>
	</owl:Class>
	
	<owl:Class rdf:about="&fibo-ind-indx-valx;InterestRateTimedValue">
		<rdfs:subClassOf rdf:resource="&fibo-ind-indx-valx;MarketParameterTimedValue"/>
		<rdfs:label xml:lang="en">interest rate timed value  (please review)</rdfs:label>
		<owl:disjointWith rdf:resource="&fibo-ind-indx-valx;ReferenceIndexDatedValue"/>
		<skos:definition xml:lang="en">The quoted value of the interest rate at the specified time and date. Term agreed; name changed from Interest Rate Value.</skos:definition>
	</owl:Class>
	
	<owl:Class rdf:about="&fibo-ind-indx-valx;MarketParameterTimedValue">
		<rdfs:subClassOf rdf:resource="&fibo-fnd-math-math;TimedValue"/>
		<rdfs:label xml:lang="en">market parameter timed value  (please review)</rdfs:label>
		<skos:definition xml:lang="en">The actual value (at a point in time) of a parameter.</skos:definition>
		<skos:editorialNote xml:lang="en">These were modeled in source model as &quot;Referenceable Archetypes&quot; (now deprecated), so there is not a hierarchy of relatjonships to these. Different types of &quot;Value&quot; with different types of qualifying terms are defined here.</skos:editorialNote>
	</owl:Class>
	
	<owl:Class rdf:about="&fibo-ind-indx-valx;ReferenceIndexDatedValue">
		<rdfs:subClassOf rdf:resource="&fibo-ind-indx-valx;MarketParameterTimedValue"/>
		<rdfs:label xml:lang="en">reference index dated value  (please review)</rdfs:label>
	</owl:Class>
	
	<owl:Class rdf:about="&fibo-ind-indx-valx;UnemploymentRateValue">
		<rdfs:subClassOf rdf:resource="&fibo-ind-indx-valx;EconomicRateQualifiedTimedValue"/>
		<rdfs:label xml:lang="en">unemployment rate value  (please review)</rdfs:label>
	</owl:Class>
	
	<owl:ObjectProperty rdf:about="&fibo-ind-indx-valx;applicablePeriod">
		<rdfs:label xml:lang="en">applicable period  (please review)</rdfs:label>
		<rdfs:domain rdf:resource="&fibo-ind-indx-valx;UnemploymentRateValue"/>
		<rdfs:range rdf:resource="&fibo-fnd-tim-tim;DatePeriod"/>
		<skos:definition xml:lang="en">The period to which the stated value of the unemployment rate applies.</skos:definition>
	</owl:ObjectProperty>
	
	<owl:ObjectProperty rdf:about="&fibo-ind-indx-valx;forYear">
		<rdfs:label xml:lang="en">for year  (please review)</rdfs:label>
		<rdfs:domain rdf:resource="&fibo-ind-indx-valx;GDPValue"/>
		<rdfs:range rdf:resource="&fibo-fnd-tim-tim;Year"/>
		<skos:definition xml:lang="en">The year for which the GDP figure applies. Further Notes Review whether this needs additional qualifying terms, e.g. the applicable year end for that country.</skos:definition>
	</owl:ObjectProperty>
	
	<owl:ObjectProperty rdf:about="&fibo-ind-indx-valx;hasGDPAmount">
		<rdfs:label xml:lang="en">has g d p amount  (please review)</rdfs:label>
		<rdfs:domain rdf:resource="&fibo-ind-indx-valx;GDPValue"/>
		<rdfs:range rdf:resource="&fibo-md-temx-tem;DatedMonetaryAmount"/>
		<skos:definition xml:lang="en">The actual value of the GDP for the applicable period, stated as a monetary amount.</skos:definition>
	</owl:ObjectProperty>
	
	<owl:ObjectProperty rdf:about="&fibo-ind-indx-valx;hasPercentageValue">
		<rdfs:label xml:lang="en">has percentage value  (please review)</rdfs:label>
		<rdfs:domain rdf:resource="&fibo-ind-indx-valx;InflationRateValue"/>
		<rdfs:range rdf:resource="&fibo-fnd-utlx-val;PercentageValue"/>
		<skos:definition xml:lang="en">The actual value of the inflation rate, stated as a percentage.</skos:definition>
	</owl:ObjectProperty>
	
	<owl:ObjectProperty rdf:about="&fibo-ind-indx-valx;hasPercentageValue.1">
		<rdfs:label xml:lang="en">has percentage value  (please review)</rdfs:label>
		<rdfs:domain rdf:resource="&fibo-ind-indx-valx;UnemploymentRateValue"/>
		<rdfs:range rdf:resource="&fibo-fnd-utlx-val;PercentageValue"/>
		<skos:definition xml:lang="en">The actual value of the unemployment rate, stated as a percentage of the population unemployed for the stated period.</skos:definition>
	</owl:ObjectProperty>
	
	<owl:ObjectProperty rdf:about="&fibo-ind-indx-valx;measurementPeriod">
		<rdfs:label xml:lang="en">measurement period  (please review)</rdfs:label>
		<rdfs:domain rdf:resource="&fibo-ind-indx-valx;InflationRateValue"/>
		<rdfs:range rdf:resource="&fibo-fnd-tim-tim;Duration"/>
		<skos:definition xml:lang="en">The period of time up to the quoted date, to which the inflation rate applies.</skos:definition>
	</owl:ObjectProperty>
	
	<owl:ObjectProperty rdf:about="&fibo-ind-indx-valx;quotedDate">
		<rdfs:label xml:lang="en">quoted date  (please review)</rdfs:label>
		<rdfs:domain rdf:resource="&fibo-ind-indx-valx;InflationRateValue"/>
		<rdfs:range rdf:resource="&fibo-fnd-dt-fd;Date"/>
		<skos:definition xml:lang="en">The date to which the quoted inflation value applies.</skos:definition>
	</owl:ObjectProperty>
	
	<owl:ObjectProperty rdf:about="&fibo-ind-indx-valx;value">
		<rdfs:label xml:lang="en">value  (please review)</rdfs:label>
		<rdfs:domain rdf:resource="&fibo-ind-indx-valx;ExchangeRateTimedValue"/>
		<rdfs:range rdf:resource="&fibo-fnd-utlx-val;DecimalValue"/>
		<skos:definition xml:lang="en">The exchange rate as a numerical ratio of the numerator to the denominator currency.</skos:definition>
	</owl:ObjectProperty>
	
	<owl:ObjectProperty rdf:about="&fibo-ind-indx-valx;value.1">
		<rdfs:label xml:lang="en">value  (please review)</rdfs:label>
		<rdfs:domain rdf:resource="&fibo-ind-indx-valx;InterestRateTimedValue"/>
		<rdfs:range rdf:resource="&fibo-fnd-utlx-val;PercentageValue"/>
		<skos:definition xml:lang="en">The quoted value of the Interest Rate at the specified time and date.</skos:definition>
	</owl:ObjectProperty>
	
	<owl:ObjectProperty rdf:about="&fibo-ind-indx-valx;value.2">
		<rdfs:label xml:lang="en">value  (please review)</rdfs:label>
		<rdfs:domain rdf:resource="&fibo-ind-indx-valx;ReferenceIndexDatedValue"/>
		<rdfs:range rdf:resource="&fibo-fnd-utlx-val;IntegerValue"/>
		<skos:definition xml:lang="en">The value of the benchmark as a number.</skos:definition>
	</owl:ObjectProperty>

</rdf:RDF>