<?xml version="1.0" encoding="UTF-8"?>
<!DOCTYPE rdf:RDF [
	<!ENTITY fibo-bp-iss-trm "https://spec.edmcouncil.org/fibo/BP/SecuritiesIssuance/IssuanceProcessTerms/">
	<!ENTITY fibo-fnd-aap-agt "https://spec.edmcouncil.org/fibo/FND/AgentsAndPeople/Agents/">
	<!ENTITY fibo-fnd-acc-cur "https://spec.edmcouncil.org/fibo/FND/Accounting/CurrencyAmount/">
	<!ENTITY fibo-fnd-agr-ctr "https://spec.edmcouncil.org/fibo/FND/Agreements/Contracts/">
	<!ENTITY fibo-fnd-arrx-mer "https://spec.edmcouncil.org/fibo/FND/Arrangements/Mereological/">
	<!ENTITY fibo-fnd-arrxx-meth "https://spec.edmcouncil.org/fibo/FND/ArrangementsExt/MethodsAndRules/">
	<!ENTITY fibo-fnd-bus-srv "https://spec.edmcouncil.org/fibo/FND/Business/Services/">
	<!ENTITY fibo-fnd-inf-inf "https://spec.edmcouncil.org/fibo/FND/Information/InfoCore/">
	<!ENTITY fibo-fnd-inf-lan "https://spec.edmcouncil.org/fibo/FND/Information/Languages/">
	<!ENTITY fibo-fnd-inf-tem "https://spec.edmcouncil.org/fibo/FND/Information/TemporalInfo/">
	<!ENTITY fibo-fnd-law-jur "https://spec.edmcouncil.org/fibo/FND/Law/Jurisdiction/">
	<!ENTITY fibo-fnd-pty-pty "https://spec.edmcouncil.org/fibo/FND/Parties/Parties/">
	<!ENTITY fibo-fnd-pub-con "https://spec.edmcouncil.org/fibo/FND/Publications/Conventions/">
	<!ENTITY fibo-fnd-rel-rel "https://spec.edmcouncil.org/fibo/FND/Relations/Relations/">
	<!ENTITY fibo-fnd-tim-tim "https://spec.edmcouncil.org/fibo/FND/Time/Time/">
	<!ENTITY fibo-fnd-txn-ecr "https://spec.edmcouncil.org/fibo/FND/Transactions/EconomicResources/">
	<!ENTITY fibo-fnd-utl-av "https://spec.edmcouncil.org/fibo/FND/Utilities/AnnotationVocabulary/">
	<!ENTITY fibo-fnd-utlx-val "https://spec.edmcouncil.org/fibo/FND/UtilitiesExt/Values/">
	<!ENTITY fibo-md-temx-ins "https://spec.edmcouncil.org/fibo/MD/TemporalCore/InstrumentTemporalTerms/">
	<!ENTITY fibo-md-temx-trs "https://spec.edmcouncil.org/fibo/MD/TemporalCore/SecurityTradingStatuses/">
	<!ENTITY fibo-sec-dbt-ab-mbs "https://spec.edmcouncil.org/fibo/SEC/Debt/AssetBacked/MortgageBackedSecurities/">
	<!ENTITY fibo-sec-secx-lisx "https://spec.edmcouncil.org/fibo/SEC/SecuritiesExt/SecuritiesListingsExt/">
	<!ENTITY fibo-sec-secx-resx "https://spec.edmcouncil.org/fibo/SEC/SecuritiesExt/SecuritiesRestrictionsExt/">
	<!ENTITY fibo-sec-secx-sec "https://spec.edmcouncil.org/fibo/SEC/SecuritiesExt/SecuritiesExt/">
	<!ENTITY fibo-sec-secx-tax "https://spec.edmcouncil.org/fibo/SEC/SecuritiesExt/SecuritiesTaxTreatment/">
	<!ENTITY fibo-uo-lat "https://spec.edmcouncil.org/fibo/UO/Lattice/">
	<!ENTITY owl "http://www.w3.org/2002/07/owl#">
	<!ENTITY rdf "http://www.w3.org/1999/02/22-rdf-syntax-ns#">
	<!ENTITY rdfs "http://www.w3.org/2000/01/rdf-schema#">
	<!ENTITY skos "http://www.w3.org/2004/02/skos/core#">
	<!ENTITY sm "http://www.omg.org/techprocess/ab/SpecificationMetadata/">
	<!ENTITY xsd "http://www.w3.org/2001/XMLSchema#">
]>
<rdf:RDF xml:base="https://spec.edmcouncil.org/fibo/SEC/SecuritiesExt/SecuritiesExt/"
	xmlns:fibo-bp-iss-trm="https://spec.edmcouncil.org/fibo/BP/SecuritiesIssuance/IssuanceProcessTerms/"
	xmlns:fibo-fnd-aap-agt="https://spec.edmcouncil.org/fibo/FND/AgentsAndPeople/Agents/"
	xmlns:fibo-fnd-acc-cur="https://spec.edmcouncil.org/fibo/FND/Accounting/CurrencyAmount/"
	xmlns:fibo-fnd-agr-ctr="https://spec.edmcouncil.org/fibo/FND/Agreements/Contracts/"
	xmlns:fibo-fnd-arrx-mer="https://spec.edmcouncil.org/fibo/FND/Arrangements/Mereological/"
	xmlns:fibo-fnd-arrxx-meth="https://spec.edmcouncil.org/fibo/FND/ArrangementsExt/MethodsAndRules/"
	xmlns:fibo-fnd-bus-srv="https://spec.edmcouncil.org/fibo/FND/Business/Services/"
	xmlns:fibo-fnd-inf-inf="https://spec.edmcouncil.org/fibo/FND/Information/InfoCore/"
	xmlns:fibo-fnd-inf-lan="https://spec.edmcouncil.org/fibo/FND/Information/Languages/"
	xmlns:fibo-fnd-inf-tem="https://spec.edmcouncil.org/fibo/FND/Information/TemporalInfo/"
	xmlns:fibo-fnd-law-jur="https://spec.edmcouncil.org/fibo/FND/Law/Jurisdiction/"
	xmlns:fibo-fnd-pty-pty="https://spec.edmcouncil.org/fibo/FND/Parties/Parties/"
	xmlns:fibo-fnd-pub-con="https://spec.edmcouncil.org/fibo/FND/Publications/Conventions/"
	xmlns:fibo-fnd-rel-rel="https://spec.edmcouncil.org/fibo/FND/Relations/Relations/"
	xmlns:fibo-fnd-tim-tim="https://spec.edmcouncil.org/fibo/FND/Time/Time/"
	xmlns:fibo-fnd-txn-ecr="https://spec.edmcouncil.org/fibo/FND/Transactions/EconomicResources/"
	xmlns:fibo-fnd-utl-av="https://spec.edmcouncil.org/fibo/FND/Utilities/AnnotationVocabulary/"
	xmlns:fibo-fnd-utlx-val="https://spec.edmcouncil.org/fibo/FND/UtilitiesExt/Values/"
	xmlns:fibo-md-temx-ins="https://spec.edmcouncil.org/fibo/MD/TemporalCore/InstrumentTemporalTerms/"
	xmlns:fibo-md-temx-trs="https://spec.edmcouncil.org/fibo/MD/TemporalCore/SecurityTradingStatuses/"
	xmlns:fibo-sec-dbt-ab-mbs="https://spec.edmcouncil.org/fibo/SEC/Debt/AssetBacked/MortgageBackedSecurities/"
	xmlns:fibo-sec-secx-lisx="https://spec.edmcouncil.org/fibo/SEC/SecuritiesExt/SecuritiesListingsExt/"
	xmlns:fibo-sec-secx-resx="https://spec.edmcouncil.org/fibo/SEC/SecuritiesExt/SecuritiesRestrictionsExt/"
	xmlns:fibo-sec-secx-sec="https://spec.edmcouncil.org/fibo/SEC/SecuritiesExt/SecuritiesExt/"
	xmlns:fibo-sec-secx-tax="https://spec.edmcouncil.org/fibo/SEC/SecuritiesExt/SecuritiesTaxTreatment/"
	xmlns:fibo-uo-lat="https://spec.edmcouncil.org/fibo/UO/Lattice/"
	xmlns:owl="http://www.w3.org/2002/07/owl#"
	xmlns:rdf="http://www.w3.org/1999/02/22-rdf-syntax-ns#"
	xmlns:rdfs="http://www.w3.org/2000/01/rdf-schema#"
	xmlns:skos="http://www.w3.org/2004/02/skos/core#"
	xmlns:sm="http://www.omg.org/techprocess/ab/SpecificationMetadata/"
	xmlns:xsd="http://www.w3.org/2001/XMLSchema#">
	
	<owl:Ontology rdf:about="https://spec.edmcouncil.org/fibo/SEC/SecuritiesExt/SecuritiesExt/">
		<rdfs:label xml:lang="en">Securities</rdfs:label>
		<owl:imports rdf:resource="http://www.omg.org/techprocess/ab/SpecificationMetadata/"/>
		<owl:imports rdf:resource="http://www.w3.org/2004/02/skos/core"/>
		<owl:imports rdf:resource="https://spec.edmcouncil.org/fibo/BP/SecuritiesIssuance/IssuanceProcessTerms/"/>
		<owl:imports rdf:resource="https://spec.edmcouncil.org/fibo/FBC/FinancialInstruments/FinancialInstruments/"/>
		<owl:imports rdf:resource="https://spec.edmcouncil.org/fibo/FND/Accounting/CurrencyAmount/"/>
		<owl:imports rdf:resource="https://spec.edmcouncil.org/fibo/FND/AgentsAndPeople/Agents/"/>
		<owl:imports rdf:resource="https://spec.edmcouncil.org/fibo/FND/Agreements/Contracts/"/>
		<owl:imports rdf:resource="https://spec.edmcouncil.org/fibo/FND/ArrangementsExt/MethodsAndRules/"/>
		<owl:imports rdf:resource="https://spec.edmcouncil.org/fibo/FND/Business/Services/"/>
		<owl:imports rdf:resource="https://spec.edmcouncil.org/fibo/FND/Information/InfoCore/"/>
		<owl:imports rdf:resource="https://spec.edmcouncil.org/fibo/FND/Information/Languages/"/>
		<owl:imports rdf:resource="https://spec.edmcouncil.org/fibo/FND/Information/TemporalInfo/"/>
		<owl:imports rdf:resource="https://spec.edmcouncil.org/fibo/FND/Law/Jurisdiction/"/>
		<owl:imports rdf:resource="https://spec.edmcouncil.org/fibo/FND/Parties/Parties/"/>
		<owl:imports rdf:resource="https://spec.edmcouncil.org/fibo/FND/Publications/Conventions/"/>
		<owl:imports rdf:resource="https://spec.edmcouncil.org/fibo/FND/Relations/Relations/"/>
		<owl:imports rdf:resource="https://spec.edmcouncil.org/fibo/FND/Time/Time/"/>
		<owl:imports rdf:resource="https://spec.edmcouncil.org/fibo/FND/Transactions/EconomicResources/"/>
		<owl:imports rdf:resource="https://spec.edmcouncil.org/fibo/FND/Utilities/AnnotationVocabulary/"/>
		<owl:imports rdf:resource="https://spec.edmcouncil.org/fibo/FND/UtilitiesExt/Values/"/>
		<owl:imports rdf:resource="https://spec.edmcouncil.org/fibo/MD/TemporalCore/InstrumentTemporalTerms/"/>
		<owl:imports rdf:resource="https://spec.edmcouncil.org/fibo/MD/TemporalCore/SecurityTradingStatuses/"/>
		<owl:imports rdf:resource="https://spec.edmcouncil.org/fibo/SEC/Debt/AssetBacked/MortgageBackedSecurities/"/>
		<owl:imports rdf:resource="https://spec.edmcouncil.org/fibo/SEC/Securities/SecuritiesIdentification/"/>
		<owl:imports rdf:resource="https://spec.edmcouncil.org/fibo/SEC/Securities/SecuritiesListings/"/>
		<owl:imports rdf:resource="https://spec.edmcouncil.org/fibo/SEC/SecuritiesExt/SecuritiesListingsExt/"/>
		<owl:imports rdf:resource="https://spec.edmcouncil.org/fibo/SEC/SecuritiesExt/SecuritiesRestrictionsExt/"/>
		<owl:imports rdf:resource="https://spec.edmcouncil.org/fibo/SEC/SecuritiesExt/SecuritiesTaxTreatment/"/>
		<owl:versionIRI rdf:resource="https://spec.edmcouncil.org/fibo/SEC/SecuritiesExt/SecuritiesExt/"/>
		<fibo-fnd-utl-av:hasMaturityLevel rdf:resource="&fibo-fnd-utl-av;Informative"/>
	</owl:Ontology>
	
	<owl:Class rdf:about="https://spec.edmcouncil.org/fibo/FBC/FinancialInstruments/FinancialInstruments/Security">
		<rdfs:subClassOf rdf:resource="&fibo-fnd-agr-ctr;TransferableContract"/>
		<rdfs:subClassOf>
			<owl:Restriction>
				<owl:onProperty rdf:resource="&fibo-sec-secx-sec;hasStructuredName"/>
				<owl:allValuesFrom rdf:resource="&fibo-sec-secx-sec;SecurityStructuredName"/>
			</owl:Restriction>
		</rdfs:subClassOf>
		<rdfs:subClassOf>
			<owl:Restriction>
				<owl:onProperty rdf:resource="&fibo-bp-iss-trm;hasIssuanceInformation"/>
				<owl:someValuesFrom rdf:resource="&fibo-bp-iss-trm;IssuedSecurityIssueInformation"/>
			</owl:Restriction>
		</rdfs:subClassOf>
		<rdfs:subClassOf>
			<owl:Restriction>
				<owl:onProperty rdf:resource="&fibo-bp-iss-trm;issuer"/>
				<owl:someValuesFrom rdf:resource="&fibo-bp-iss-trm;SecurityIssuer"/>
			</owl:Restriction>
		</rdfs:subClassOf>
		<rdfs:subClassOf>
			<owl:Restriction>
				<owl:onProperty rdf:resource="&fibo-fnd-inf-tem;hasStatus"/>
				<owl:someValuesFrom rdf:resource="&fibo-md-temx-trs;SecurityLifecycleStatus"/>
			</owl:Restriction>
		</rdfs:subClassOf>
		<rdfs:subClassOf>
			<owl:Restriction>
				<owl:onProperty rdf:resource="&fibo-md-temx-ins;hasPrice"/>
				<owl:someValuesFrom rdf:resource="&fibo-md-temx-ins;TradedSecurityPublishedPrice"/>
			</owl:Restriction>
		</rdfs:subClassOf>
		<rdfs:subClassOf>
			<owl:Restriction>
				<owl:onProperty rdf:resource="&fibo-sec-secx-sec;denominationCurrency"/>
				<owl:someValuesFrom rdf:resource="&fibo-fnd-acc-cur;Currency"/>
			</owl:Restriction>
		</rdfs:subClassOf>
		<rdfs:subClassOf>
			<owl:Restriction>
				<owl:onProperty rdf:resource="&fibo-sec-secx-sec;hasDefaultSettlementTerms"/>
				<owl:someValuesFrom rdf:resource="&fibo-sec-secx-sec;SecuritySettlementConvention"/>
			</owl:Restriction>
		</rdfs:subClassOf>
		<rdfs:subClassOf>
			<owl:Restriction>
				<owl:onProperty rdf:resource="&fibo-sec-secx-sec;hasStructuredName"/>
				<owl:someValuesFrom rdf:resource="&fibo-sec-secx-sec;SecurityStructuredName"/>
			</owl:Restriction>
		</rdfs:subClassOf>
		<rdfs:subClassOf>
			<owl:Restriction>
				<owl:onProperty rdf:resource="&fibo-sec-secx-sec;legallyRecordedIn"/>
				<owl:someValuesFrom rdf:resource="&fibo-fnd-law-jur;Jurisdiction"/>
			</owl:Restriction>
		</rdfs:subClassOf>
		<rdfs:subClassOf>
			<owl:Restriction>
				<owl:onProperty rdf:resource="&fibo-sec-secx-tax;hasTaxTreatment"/>
				<owl:someValuesFrom rdf:resource="&fibo-sec-secx-tax;SecurityTaxTreatment"/>
			</owl:Restriction>
		</rdfs:subClassOf>
		<rdfs:label xml:lang="en">security</rdfs:label>
		<owl:equivalentClass rdf:resource="https://spec.edmcouncil.org/fibo/FBC/FinancialInstruments/FinancialInstruments/Security"/>
		<skos:definition xml:lang="en">A financial instrument which can be bought or sold. This may be traded either over the counter or through an exchange or other trading venue.</skos:definition>
		<fibo-fnd-utl-av:explanatoryNote xml:lang="en">This is a publicly traded security (corresponding to the scope of &quot;Security&quot; in ISO 20022) and therefore does not include privately held equity or equity in companies that are not publicly traded.</fibo-fnd-utl-av:explanatoryNote>
	</owl:Class>
	
	<owl:Class rdf:about="https://spec.edmcouncil.org/fibo/SEC/Securities/SecuritiesListings/ExchangeTradedSecurity">
		<rdfs:subClassOf rdf:resource="&fibo-sec-secx-sec;TradingRegisteredSecurity"/>
		<rdfs:subClassOf>
			<owl:Restriction>
				<owl:onProperty rdf:resource="&fibo-sec-secx-resx;hasRestrictions"/>
				<owl:someValuesFrom rdf:resource="&fibo-sec-secx-resx;InvestmentRestriction"/>
			</owl:Restriction>
		</rdfs:subClassOf>
		<skos:definition xml:lang="en">Tradable security traded on an exchange or other trading venue.</skos:definition>
	</owl:Class>
	
	<owl:Class rdf:about="&fibo-sec-secx-sec;CashSecuritiesDelivery">
		<rdfs:subClassOf rdf:resource="&fibo-sec-secx-sec;SecurityDeliveryType"/>
		<rdfs:label xml:lang="en">cash securities delivery</rdfs:label>
		<skos:definition xml:lang="en">Delivery of a security in cash</skos:definition>
	</owl:Class>
	
	<owl:Class rdf:about="&fibo-sec-secx-sec;NonCashSecuritiesDelivery">
		<rdfs:subClassOf rdf:resource="&fibo-sec-secx-sec;SecurityDeliveryType"/>
		<rdfs:label xml:lang="en">non cash securities delivery</rdfs:label>
		<skos:definition xml:lang="en">Delivery is by some other means.</skos:definition>
		<skos:editorialNote xml:lang="en">Review: There may be more applicable values for this selection. Used in settlement terms and (if required) in settlement conventions for the security.</skos:editorialNote>
	</owl:Class>
	
	<owl:Class rdf:about="&fibo-sec-secx-sec;SecurityContractTerms">
		<rdfs:subClassOf rdf:resource="&fibo-fnd-agr-ctr;ContractualCommitment"/>
		<rdfs:label xml:lang="en">security contract terms</rdfs:label>
		<skos:definition xml:lang="en">Contractual terms of a negotiable financial security</skos:definition>
	</owl:Class>
	
	<owl:Class rdf:about="&fibo-sec-secx-sec;SecurityDeliveryType">
		<rdfs:subClassOf rdf:resource="&fibo-fnd-arrxx-meth;DeliveryMethod"/>
		<rdfs:label xml:lang="en">security delivery type  (please review)</rdfs:label>
		<skos:definition xml:lang="en">Type of delivery as used in settlement terms for a financial security.</skos:definition>
	</owl:Class>
	
	<owl:Class rdf:about="&fibo-sec-secx-sec;SecurityNote">
		<rdfs:label xml:lang="en">security note  (please review)</rdfs:label>
		<skos:definition xml:lang="en">An individually denominated note within a security or tranche of a security, where this is issued in notes of different denominations.</skos:definition>
		<skos:editorialNote xml:lang="en">Introduced for MBS Proof of Concept, to model MBS tranches where one tranche may have notes of multiple denominations. Other applications of this concept are not known at present. Trivially, all securities could be said to be in &quot;notes&quot; in this sense but the term is not normally referred to.</skos:editorialNote>
	</owl:Class>
	
	<owl:Class rdf:about="&fibo-sec-secx-sec;SecuritySettlementConvention">
		<rdfs:subClassOf rdf:resource="&fibo-sec-secx-sec;SettlementConvention"/>
		<rdfs:subClassOf>
			<owl:Restriction>
				<owl:onProperty rdf:resource="&fibo-sec-secx-sec;hasDeliveryMethod"/>
				<owl:someValuesFrom rdf:resource="&fibo-sec-secx-sec;SecurityDeliveryType"/>
			</owl:Restriction>
		</rdfs:subClassOf>
		<rdfs:label xml:lang="en">security settlement convention</rdfs:label>
		<skos:definition xml:lang="en">Default Terms for the settlement of a Security.</skos:definition>
	</owl:Class>
	
	<owl:Class rdf:about="&fibo-sec-secx-sec;SecurityStructuredName">
		<rdfs:subClassOf rdf:resource="&fibo-fnd-inf-inf;StructuredName"/>
		<rdfs:label xml:lang="en">security structured name</rdfs:label>
		<skos:definition xml:lang="en">The formal, structured name of a Security.</skos:definition>
	</owl:Class>
	
	<owl:Class rdf:about="&fibo-sec-secx-sec;SettlementConvention">
		<rdfs:subClassOf rdf:resource="&fibo-fnd-pub-con;Convention"/>
		<rdfs:label xml:lang="en">settlement convention</rdfs:label>
		<skos:definition xml:lang="en">A convention for settlement of a trade or transaction.</skos:definition>
		<fibo-fnd-utl-av:explanatoryNote xml:lang="en">This is usually stated in the form &apos;T+n&apos; where n is the Settlement Business Days. There are no date roll rules, the T+n simply refers to the next available business days and is specified as a whole number. Note that this term has been created for the OTC model, but on review of the existing terms for security settlement conventions in the common model for tradable securities, this term has been separated out as a more general term, with the securities-specific in a sub-type of this item, renamed to Security Settlement Convention.</fibo-fnd-utl-av:explanatoryNote>
	</owl:Class>
	
	<owl:Class rdf:about="&fibo-sec-secx-sec;Stake">
		<rdfs:label xml:lang="en">stake</rdfs:label>
		<skos:definition xml:lang="en">The holding of some portion of some venture or something of value, by some party. The stake may be represented by some form of formal document such as a share or some debt unit.</skos:definition>
	</owl:Class>
	
	<owl:Class rdf:about="&fibo-sec-secx-sec;TradingRegisteredSecurity">
		<rdfs:subClassOf rdf:resource="https://spec.edmcouncil.org/fibo/FBC/FinancialInstruments/FinancialInstruments/Security"/>
		<rdfs:subClassOf>
			<owl:Restriction>
				<owl:onProperty rdf:resource="https://spec.edmcouncil.org/fibo/SEC/Equities/ShareTerms/hasListing"/>
				<owl:someValuesFrom rdf:resource="https://spec.edmcouncil.org/fibo/SEC/Securities/SecuritiesListings/SecurityListing"/>
			</owl:Restriction>
		</rdfs:subClassOf>
		<rdfs:label xml:lang="en">trading registered security</rdfs:label>
		<skos:definition xml:lang="en">A security which is traded on some trading venue.</skos:definition>
		<skos:editorialNote xml:lang="en">Define the three types of these as per the MIFID definitions of types of trading facility. Also need to allow for jurisdiction variation. Renamed March 2013 from Listed Security to Trading Registered Security (Citi review session). The rationale is that any security which is listed on some facility is registered, and the fact of it being registered is more significant. This is still to be reviewed more widely with the SME review group.</skos:editorialNote>
	</owl:Class>
	
	<owl:ObjectProperty rdf:about="&fibo-sec-secx-sec;allowsContractualSettlement">
		<rdfs:label xml:lang="en">allows contractual settlement  (please review)</rdfs:label>
		<rdfs:domain rdf:resource="&fibo-sec-secx-sec;SecuritySettlementConvention"/>
		<rdfs:range rdf:resource="&fibo-fnd-utlx-val;TrueFalseValue"/>
		<skos:definition xml:lang="en">Whether the market allows contractual settlement. This is a settlement term related to the market.</skos:definition>
	</owl:ObjectProperty>
	
	<owl:ObjectProperty rdf:about="&fibo-sec-secx-sec;bearer">
		<rdfs:label xml:lang="en">bearer  (please review)</rdfs:label>
		<rdfs:domain rdf:resource="https://spec.edmcouncil.org/fibo/FBC/FinancialInstruments/FinancialInstruments/Security"/>
		<rdfs:range rdf:resource="&fibo-fnd-utlx-val;TrueFalseValue"/>
		<skos:definition xml:lang="en">The owner is not registered in the books of the issuer or of the registrar.</skos:definition>
	</owl:ObjectProperty>
	
	<owl:ObjectProperty rdf:about="&fibo-sec-secx-sec;deemedRiskCurrency">
		<rdfs:label xml:lang="en">deemed risk currency  (please review)</rdfs:label>
		<rdfs:domain rdf:resource="https://spec.edmcouncil.org/fibo/FBC/FinancialInstruments/FinancialInstruments/Security"/>
		<rdfs:range rdf:resource="&fibo-fnd-acc-cur;Currency"/>
		<skos:definition xml:lang="en">The currency in which any risks relating to the instrument are seen to take place. Further notes: This is a risk specific term identified during SME Reviews of common securities terms. It was agreed at a review with a risk firm that this term is applicable within the context of risk management only and is not a fundamental fact about the security. It therefore needs to be disposed in some way to show it in the context of risk.</skos:definition>
	</owl:ObjectProperty>
	
	<owl:ObjectProperty rdf:about="&fibo-sec-secx-sec;denominationCurrency">
		<rdfs:label xml:lang="en">denomination currency  (please review)</rdfs:label>
		<rdfs:domain rdf:resource="https://spec.edmcouncil.org/fibo/FBC/FinancialInstruments/FinancialInstruments/Security"/>
		<rdfs:range rdf:resource="&fibo-fnd-acc-cur;Currency"/>
		<skos:definition xml:lang="en">The default currency in which units of the Security are denominated.</skos:definition>
	</owl:ObjectProperty>
	
	<owl:ObjectProperty rdf:about="&fibo-sec-secx-sec;denominationIncrement">
		<rdfs:label xml:lang="en">denomination increment  (please review)</rdfs:label>
		<rdfs:domain rdf:resource="https://spec.edmcouncil.org/fibo/FBC/FinancialInstruments/FinancialInstruments/Security"/>
		<rdfs:range rdf:resource="&fibo-fnd-utlx-val;IntegerValue"/>
		<skos:definition xml:lang="en">The multiples above the smallest possible denomination (Default Lot Size) in which the security can be held.</skos:definition>
	</owl:ObjectProperty>
	
	<owl:ObjectProperty rdf:about="&fibo-sec-secx-sec;fASTApplicable">
		<rdfs:label xml:lang="en">f a s t applicable  (please review)</rdfs:label>
		<rdfs:domain rdf:resource="https://spec.edmcouncil.org/fibo/FBC/FinancialInstruments/FinancialInstruments/Security"/>
		<rdfs:range rdf:resource="&fibo-fnd-utlx-val;TrueFalseValue"/>
		<skos:definition xml:lang="en">Whether the security is to be held at the transfer agent as part of the FAST (Fully Automated Securities Transfer) program. Further notes: Term is specific to DTCC / US context. Is there a more generic meaning similar to this which applies across different jurisdictions? If not this term should be defined with reference to this specific context.</skos:definition>
	</owl:ObjectProperty>
	
	<owl:ObjectProperty rdf:about="&fibo-sec-secx-sec;fractionalEligible">
		<rdfs:label xml:lang="en">fractional eligible  (please review)</rdfs:label>
		<rdfs:domain rdf:resource="https://spec.edmcouncil.org/fibo/FBC/FinancialInstruments/FinancialInstruments/Security"/>
		<rdfs:range rdf:resource="&fibo-fnd-utlx-val;TrueFalseValue"/>
		<skos:definition xml:lang="en">Whether the security can contain Fractional Share/amount component.</skos:definition>
	</owl:ObjectProperty>
	
	<owl:ObjectProperty rdf:about="&fibo-sec-secx-sec;fullName">
		<rdfs:label xml:lang="en">full name  (please review)</rdfs:label>
		<rdfs:domain rdf:resource="&fibo-sec-secx-sec;SecurityStructuredName"/>
		<rdfs:range rdf:resource="&fibo-fnd-utlx-val;TextValue"/>
		<skos:definition xml:lang="en">Full name of the security</skos:definition>
	</owl:ObjectProperty>
	
	<owl:ObjectProperty rdf:about="&fibo-sec-secx-sec;hasDefaultSettlementTerms">
		<rdfs:label xml:lang="en">has default settlement terms  (please review)</rdfs:label>
		<rdfs:domain rdf:resource="https://spec.edmcouncil.org/fibo/FBC/FinancialInstruments/FinancialInstruments/Security"/>
		<rdfs:range rdf:resource="&fibo-sec-secx-sec;SecuritySettlementConvention"/>
	</owl:ObjectProperty>
	
	<owl:ObjectProperty rdf:about="&fibo-sec-secx-sec;hasDeliveryMethod">
		<rdfs:label xml:lang="en">has delivery method  (please review)</rdfs:label>
		<rdfs:domain rdf:resource="&fibo-sec-secx-sec;SecuritySettlementConvention"/>
		<rdfs:range rdf:resource="&fibo-sec-secx-sec;SecurityDeliveryType"/>
		<skos:definition xml:lang="en">Has a method by which securities are delivered at settlement.</skos:definition>
	</owl:ObjectProperty>
	
	<owl:ObjectProperty rdf:about="&fibo-sec-secx-sec;hasStructuredName">
		<rdfs:subPropertyOf rdf:resource="&fibo-fnd-inf-inf;hasName"/>
		<rdfs:label xml:lang="en">has structured name</rdfs:label>
		<rdfs:domain rdf:resource="https://spec.edmcouncil.org/fibo/FBC/FinancialInstruments/FinancialInstruments/Security"/>
		<rdfs:range rdf:resource="&fibo-sec-secx-sec;SecurityStructuredName"/>
	</owl:ObjectProperty>
	
	<owl:ObjectProperty rdf:about="&fibo-sec-secx-sec;interchangeable">
		<rdfs:label xml:lang="en">interchangeable  (please review)</rdfs:label>
		<rdfs:domain rdf:resource="https://spec.edmcouncil.org/fibo/FBC/FinancialInstruments/FinancialInstruments/Security"/>
		<rdfs:range rdf:resource="&fibo-fnd-utlx-val;TrueFalseValue"/>
		<skos:definition xml:lang="en">Whether or not the security is freely interchangeable with other of the same securities. Yes indicates that the security is interchangeable; no indicates that it is not.</skos:definition>
	</owl:ObjectProperty>
	
	<owl:ObjectProperty rdf:about="&fibo-sec-secx-sec;isListed">
		<rdfs:label xml:lang="en">is listed  (please review)</rdfs:label>
		<rdfs:domain rdf:resource="&fibo-sec-secx-sec;TradingRegisteredSecurity"/>
		<rdfs:range rdf:resource="&fibo-fnd-utlx-val;TrueFalseValue"/>
		<skos:definition xml:lang="en">The security is listed on some exchange or trading facility (Listed = Yes)</skos:definition>
	</owl:ObjectProperty>
	
	<owl:ObjectProperty rdf:about="&fibo-sec-secx-sec;issueDate">
		<rdfs:label xml:lang="en">issue date  (please review)</rdfs:label>
		<rdfs:domain rdf:resource="https://spec.edmcouncil.org/fibo/FBC/FinancialInstruments/FinancialInstruments/Security"/>
		<rdfs:range rdf:resource="&fibo-fnd-tim-tim;Date"/>
		<skos:definition xml:lang="en">Date that the Security was issued.</skos:definition>
	</owl:ObjectProperty>
	
	<owl:ObjectProperty rdf:about="&fibo-sec-secx-sec;legallyRecordedIn">
		<rdfs:subPropertyOf rdf:resource="&fibo-fnd-agr-ctr;hasGoverningJurisdiction"/>
		<rdfs:label xml:lang="en">legally recorded in  (please review)</rdfs:label>
		<rdfs:domain rdf:resource="https://spec.edmcouncil.org/fibo/FBC/FinancialInstruments/FinancialInstruments/Security"/>
		<rdfs:range rdf:resource="&fibo-fnd-law-jur;Jurisdiction"/>
		<skos:definition xml:lang="en">Jurisdiction (country, county, state, province, city) in which the security is legally recorded for regulatory and/or tax purposes.</skos:definition>
	</owl:ObjectProperty>
	
	<owl:ObjectProperty rdf:about="&fibo-sec-secx-sec;listed">
		<rdfs:label xml:lang="en">listed  (please review)</rdfs:label>
		<rdfs:domain rdf:resource="https://spec.edmcouncil.org/fibo/FBC/FinancialInstruments/FinancialInstruments/Security"/>
		<rdfs:range rdf:resource="&fibo-fnd-utlx-val;TrueFalseValue"/>
		<skos:definition xml:lang="en">Whether or not the security is listed on some exchange or trading facility.</skos:definition>
	</owl:ObjectProperty>
	
	<owl:ObjectProperty rdf:about="&fibo-sec-secx-sec;preferredSettlementCurrency">
		<rdfs:label xml:lang="en">preferred settlement currency  (please review)</rdfs:label>
		<rdfs:domain rdf:resource="&fibo-sec-secx-sec;SecuritySettlementConvention"/>
		<rdfs:range rdf:resource="&fibo-fnd-acc-cur;Currency"/>
		<skos:definition xml:lang="en">Preferred currency in which the instrument is to be settled. Securities may be settled in a currency other than this.</skos:definition>
	</owl:ObjectProperty>
	
	<owl:ObjectProperty rdf:about="&fibo-sec-secx-sec;registered">
		<rdfs:label xml:lang="en">registered  (please review)</rdfs:label>
		<rdfs:domain rdf:resource="https://spec.edmcouncil.org/fibo/FBC/FinancialInstruments/FinancialInstruments/Security"/>
		<rdfs:range rdf:resource="&fibo-fnd-utlx-val;TrueFalseValue"/>
		<skos:definition xml:lang="en">Securities are recorded in the name of the owner on the books of the issuer or the issuer&apos;s registrar.</skos:definition>
	</owl:ObjectProperty>
	
	<owl:ObjectProperty rdf:about="&fibo-sec-secx-sec;settlementBusinessDays">
		<rdfs:label xml:lang="en">settlement business days  (please review)</rdfs:label>
		<rdfs:domain rdf:resource="&fibo-sec-secx-sec;SettlementConvention"/>
		<rdfs:range rdf:resource="&fibo-fnd-utlx-val;IntegerValue"/>
		<skos:definition xml:lang="en">Default number of business days for settlement e.g. T+1, T+3 and so on.</skos:definition>
	</owl:ObjectProperty>
	
	<owl:ObjectProperty rdf:about="&fibo-sec-secx-sec;shortName">
		<rdfs:label xml:lang="en">short name  (please review)</rdfs:label>
		<rdfs:domain rdf:resource="&fibo-sec-secx-sec;SecurityStructuredName"/>
		<rdfs:range rdf:resource="&fibo-fnd-utlx-val;TextValue"/>
		<skos:definition xml:lang="en">Short name of the security.</skos:definition>
	</owl:ObjectProperty>

</rdf:RDF>