<?xml version="1.0" encoding="UTF-8"?>
<!DOCTYPE rdf:RDF [
	<!ENTITY fibo-fnd-accx-tax "https://spec.edmcouncil.org/fibo/FND/AccountingExt/Taxation/">
	<!ENTITY fibo-fnd-utl-av "https://spec.edmcouncil.org/fibo/FND/Utilities/AnnotationVocabulary/">
	<!ENTITY fibo-fnd-utlx-val "https://spec.edmcouncil.org/fibo/FND/UtilitiesExt/Values/">
	<!ENTITY fibo-sec-secx-tax "https://spec.edmcouncil.org/fibo/SEC/SecuritiesExt/SecuritiesTaxTreatment/">
	<!ENTITY owl "http://www.w3.org/2002/07/owl#">
	<!ENTITY rdf "http://www.w3.org/1999/02/22-rdf-syntax-ns#">
	<!ENTITY rdfs "http://www.w3.org/2000/01/rdf-schema#">
	<!ENTITY skos "http://www.w3.org/2004/02/skos/core#">
	<!ENTITY xsd "http://www.w3.org/2001/XMLSchema#">
]>
<rdf:RDF xml:base="https://spec.edmcouncil.org/fibo/SEC/SecuritiesExt/SecuritiesTaxTreatment/"
	xmlns:fibo-fnd-accx-tax="https://spec.edmcouncil.org/fibo/FND/AccountingExt/Taxation/"
	xmlns:fibo-fnd-utl-av="https://spec.edmcouncil.org/fibo/FND/Utilities/AnnotationVocabulary/"
	xmlns:fibo-fnd-utlx-val="https://spec.edmcouncil.org/fibo/FND/UtilitiesExt/Values/"
	xmlns:fibo-sec-secx-tax="https://spec.edmcouncil.org/fibo/SEC/SecuritiesExt/SecuritiesTaxTreatment/"
	xmlns:owl="http://www.w3.org/2002/07/owl#"
	xmlns:rdf="http://www.w3.org/1999/02/22-rdf-syntax-ns#"
	xmlns:rdfs="http://www.w3.org/2000/01/rdf-schema#"
	xmlns:skos="http://www.w3.org/2004/02/skos/core#"
	xmlns:xsd="http://www.w3.org/2001/XMLSchema#">
	
	<owl:Ontology rdf:about="https://spec.edmcouncil.org/fibo/SEC/SecuritiesExt/SecuritiesTaxTreatment/">
		<rdfs:label xml:lang="en">SecuritiesTaxTreatment</rdfs:label>
		<owl:imports rdf:resource="http://www.w3.org/2004/02/skos/core"/>
		<owl:imports rdf:resource="https://spec.edmcouncil.org/fibo/FBC/FinancialInstruments/FinancialInstruments/"/>
		<owl:imports rdf:resource="https://spec.edmcouncil.org/fibo/FND/AccountingExt/Taxation/"/>
		<owl:imports rdf:resource="https://spec.edmcouncil.org/fibo/FND/Utilities/AnnotationVocabulary/"/>
		<owl:imports rdf:resource="https://spec.edmcouncil.org/fibo/FND/UtilitiesExt/Values/"/>
		<owl:versionIRI rdf:resource="https://spec.edmcouncil.org/fibo/SEC/SecuritiesExt/SecuritiesTaxTreatment/"/>
		<fibo-fnd-utl-av:hasMaturityLevel rdf:resource="&fibo-fnd-utl-av;Informative"/>
	</owl:Ontology>
	
	<owl:Class rdf:about="https://spec.edmcouncil.org/fibo/FBC/FinancialInstruments/FinancialInstruments/FinancialInstrument">
	</owl:Class>
	
	<owl:Class rdf:about="&fibo-sec-secx-tax;FinancialInstrumentTaxTreatment">
		<rdfs:subClassOf rdf:resource="&fibo-fnd-accx-tax;TaxTreatment"/>
		<rdfs:label xml:lang="en">financial instrument tax treatment  (please review)</rdfs:label>
		<skos:definition xml:lang="en">The treatment of the financial instrument for taxation purposes. This is the most general form of tax treatment for financial instruments, including cash.</skos:definition>
	</owl:Class>
	
	<owl:Class rdf:about="&fibo-sec-secx-tax;SecurityTaxTreatment">
		<rdfs:subClassOf rdf:resource="&fibo-sec-secx-tax;FinancialInstrumentTaxTreatment"/>
		<rdfs:label xml:lang="en">security tax treatment  (please review)</rdfs:label>
		<skos:definition xml:lang="en">Amount of money due to the government or tax authority, according to various pre-defined parameters such as thresholds or income.</skos:definition>
	</owl:Class>
	
	<owl:ObjectProperty rdf:about="&fibo-sec-secx-tax;exempt">
		<rdfs:label xml:lang="en">exempt  (please review)</rdfs:label>
		<rdfs:domain rdf:resource="&fibo-sec-secx-tax;FinancialInstrumentTaxTreatment"/>
		<rdfs:range rdf:resource="&fibo-fnd-utlx-val;TrueFalseValue"/>
		<skos:definition xml:lang="en">Whether the tax rule applies within the jurisdiction as a condition of this instrument.</skos:definition>
	</owl:ObjectProperty>
	
	<owl:ObjectProperty rdf:about="&fibo-sec-secx-tax;frankedRate">
		<rdfs:label xml:lang="en">franked rate  (please review)</rdfs:label>
		<rdfs:domain rdf:resource="&fibo-sec-secx-tax;SecurityTaxTreatment"/>
		<rdfs:range rdf:resource="&fibo-fnd-utlx-val;PercentageValue"/>
		<skos:definition xml:lang="en">Percentage of dividend for which tax is already paid.</skos:definition>
	</owl:ObjectProperty>
	
	<owl:ObjectProperty rdf:about="&fibo-sec-secx-tax;hasTaxTreatment">
		<rdfs:label xml:lang="en">has tax treatment  (please review)</rdfs:label>
		<rdfs:domain rdf:resource="https://spec.edmcouncil.org/fibo/FBC/FinancialInstruments/FinancialInstruments/FinancialInstrument"/>
		<rdfs:range rdf:resource="&fibo-sec-secx-tax;FinancialInstrumentTaxTreatment"/>
	</owl:ObjectProperty>
	
	<owl:ObjectProperty rdf:about="&fibo-sec-secx-tax;securityTaxCode">
		<rdfs:label xml:lang="en">security tax code  (please review)</rdfs:label>
		<rdfs:domain rdf:resource="&fibo-sec-secx-tax;SecurityTaxTreatment"/>
		<rdfs:range rdf:resource="&fibo-fnd-utlx-val;TextValue"/>
		<skos:definition xml:lang="en">The tax code of the security in the stated tax jurisdiction.</skos:definition>
	</owl:ObjectProperty>

</rdf:RDF>