<?xml version="1.0" encoding="UTF-8"?>
<!DOCTYPE rdf:RDF [
	<!ENTITY fibo-be-le-fbo "https://spec.edmcouncil.org/fibo/BE/LegalEntities/FormalBusinessOrganizations/">
	<!ENTITY fibo-fnd-arr-cls "https://spec.edmcouncil.org/fibo/FND/Arrangements/ClassificationSchemes/">
	<!ENTITY fibo-fnd-rel-rel "https://spec.edmcouncil.org/fibo/FND/Relations/Relations/">
	<!ENTITY fibo-fnd-utl-av "https://spec.edmcouncil.org/fibo/FND/Utilities/AnnotationVocabulary/">
	<!ENTITY fibo-sec-secx-clax "https://spec.edmcouncil.org/fibo/SEC/SecuritiesExt/SecuritiesClassificationExt/">
	<!ENTITY owl "http://www.w3.org/2002/07/owl#">
	<!ENTITY rdf "http://www.w3.org/1999/02/22-rdf-syntax-ns#">
	<!ENTITY rdfs "http://www.w3.org/2000/01/rdf-schema#">
	<!ENTITY skos "http://www.w3.org/2004/02/skos/core#">
	<!ENTITY xsd "http://www.w3.org/2001/XMLSchema#">
]>
<rdf:RDF xml:base="https://spec.edmcouncil.org/fibo/SEC/SecuritiesExt/SecuritiesClassificationExt/"
	xmlns:fibo-be-le-fbo="https://spec.edmcouncil.org/fibo/BE/LegalEntities/FormalBusinessOrganizations/"
	xmlns:fibo-fnd-arr-cls="https://spec.edmcouncil.org/fibo/FND/Arrangements/ClassificationSchemes/"
	xmlns:fibo-fnd-rel-rel="https://spec.edmcouncil.org/fibo/FND/Relations/Relations/"
	xmlns:fibo-fnd-utl-av="https://spec.edmcouncil.org/fibo/FND/Utilities/AnnotationVocabulary/"
	xmlns:fibo-sec-secx-clax="https://spec.edmcouncil.org/fibo/SEC/SecuritiesExt/SecuritiesClassificationExt/"
	xmlns:owl="http://www.w3.org/2002/07/owl#"
	xmlns:rdf="http://www.w3.org/1999/02/22-rdf-syntax-ns#"
	xmlns:rdfs="http://www.w3.org/2000/01/rdf-schema#"
	xmlns:skos="http://www.w3.org/2004/02/skos/core#"
	xmlns:xsd="http://www.w3.org/2001/XMLSchema#">
	
	<owl:Ontology rdf:about="https://spec.edmcouncil.org/fibo/SEC/SecuritiesExt/SecuritiesClassificationExt/">
		<rdfs:label xml:lang="en">SecuritiesClassificationExt</rdfs:label>
		<owl:imports rdf:resource="http://www.w3.org/2004/02/skos/core"/>
		<owl:imports rdf:resource="https://spec.edmcouncil.org/fibo/BE/LegalEntities/FormalBusinessOrganizations/"/>
		<owl:imports rdf:resource="https://spec.edmcouncil.org/fibo/FBC/FinancialInstruments/FinancialInstruments/"/>
		<owl:imports rdf:resource="https://spec.edmcouncil.org/fibo/FND/Arrangements/ClassificationSchemes/"/>
		<owl:imports rdf:resource="https://spec.edmcouncil.org/fibo/FND/Relations/Relations/"/>
		<owl:imports rdf:resource="https://spec.edmcouncil.org/fibo/FND/Utilities/AnnotationVocabulary/"/>
		<owl:imports rdf:resource="https://spec.edmcouncil.org/fibo/SEC/Securities/SecuritiesClassification/"/>
		<fibo-fnd-utl-av:hasMaturityLevel rdf:resource="&fibo-fnd-utl-av;Informative"/>
	</owl:Ontology>
	
	<owl:Class rdf:about="https://spec.edmcouncil.org/fibo/FBC/FinancialInstruments/FinancialInstruments/Security">
		<rdfs:subClassOf>
			<owl:Restriction>
				<owl:onProperty rdf:resource="&fibo-fnd-rel-rel;isClassifiedBy"/>
				<owl:someValuesFrom rdf:resource="&fibo-sec-secx-clax;SecurityClassification"/>
			</owl:Restriction>
		</rdfs:subClassOf>
		<rdfs:subClassOf>
			<owl:Restriction>
				<owl:onProperty rdf:resource="&fibo-sec-secx-clax;hasSectorClassification"/>
				<owl:someValuesFrom rdf:resource="&fibo-fnd-arr-cls;IndustrySectorClassifier"/>
			</owl:Restriction>
		</rdfs:subClassOf>
		<rdfs:label xml:lang="en">security</rdfs:label>
		<owl:equivalentClass rdf:resource="https://spec.edmcouncil.org/fibo/FBC/FinancialInstruments/FinancialInstruments/Security"/>
	</owl:Class>
	
	<owl:Class rdf:about="&fibo-fnd-arr-cls;IndustrySectorClassifier">
		<rdfs:subClassOf>
			<owl:Restriction>
				<owl:onProperty rdf:resource="&fibo-fnd-rel-rel;classifies"/>
				<owl:someValuesFrom rdf:resource="&fibo-be-le-fbo;FormallyConstitutedOrganization"/>
			</owl:Restriction>
		</rdfs:subClassOf>
		<rdfs:label xml:lang="en">industry sector classifier</rdfs:label>
		<owl:equivalentClass rdf:resource="&fibo-fnd-arr-cls;IndustrySectorClassifier"/>
		<skos:definition xml:lang="en">An Industry Sector Classification, identifying industries according to some Scheme. This may be applied to a Security, an Organization or some other thing or activity.</skos:definition>
	</owl:Class>
	
	<owl:Class rdf:about="&fibo-sec-secx-clax;SectorClassificationScheme">
		<rdfs:subClassOf rdf:resource="&fibo-fnd-arr-cls;ClassificationScheme"/>
		<rdfs:subClassOf>
			<owl:Restriction>
				<owl:onProperty rdf:resource="&fibo-fnd-rel-rel;defines"/>
				<owl:someValuesFrom rdf:resource="&fibo-fnd-arr-cls;IndustrySectorClassifier"/>
			</owl:Restriction>
		</rdfs:subClassOf>
		<rdfs:label xml:lang="en">sector classification scheme</rdfs:label>
		<skos:definition xml:lang="en">Scheme defining the structure and semantics of a set of classification codes which identify different industry sectors and (optionally) sub-sectors.</skos:definition>
	</owl:Class>
	
	<owl:Class rdf:about="&fibo-sec-secx-clax;SecurityClassification">
		<rdfs:subClassOf rdf:resource="https://spec.edmcouncil.org/fibo/SEC/Securities/SecuritiesClassification/FinancialInstrumentClassifier"/>
		<rdfs:label xml:lang="en">security classification</rdfs:label>
		<skos:definition xml:lang="en">The classification of the type of security, e.g. Equity, Debt, Short Term Note etc.</skos:definition>
		<fibo-fnd-utl-av:explanatoryNote xml:lang="en">Not the same as the Industry Classification identifying the industry sector associated with the Security.</fibo-fnd-utl-av:explanatoryNote>
	</owl:Class>
	
	<owl:Class rdf:about="&fibo-sec-secx-clax;SecurityClassificationScheme">
		<rdfs:subClassOf rdf:resource="https://spec.edmcouncil.org/fibo/SEC/Securities/SecuritiesClassification/FinancialInstrumentClassificationScheme"/>
		<rdfs:subClassOf>
			<owl:Restriction>
				<owl:onProperty rdf:resource="&fibo-fnd-rel-rel;defines"/>
				<owl:allValuesFrom rdf:resource="&fibo-sec-secx-clax;SecurityClassification"/>
			</owl:Restriction>
		</rdfs:subClassOf>
		<rdfs:label xml:lang="en">security classification scheme</rdfs:label>
		<skos:definition xml:lang="en">The Scheme defining the classification of a security i..e what type of security it is (for example the ISO 10962 CFI lassification Scheme). This may be referred to by means of a URI or some other means depending on the convention adopted on implementation.</skos:definition>
	</owl:Class>
	
	<owl:ObjectProperty rdf:about="&fibo-sec-secx-clax;hasSectorClassification">
		<rdfs:subPropertyOf rdf:resource="&fibo-fnd-rel-rel;isClassifiedBy"/>
		<rdfs:label xml:lang="en">has sector classification</rdfs:label>
		<rdfs:domain rdf:resource="https://spec.edmcouncil.org/fibo/FBC/FinancialInstruments/FinancialInstruments/Security"/>
		<rdfs:range rdf:resource="&fibo-fnd-arr-cls;IndustrySectorClassifier"/>
	</owl:ObjectProperty>

</rdf:RDF>