<?xml version="1.0" encoding="UTF-8"?>
  
<!DOCTYPE rdf:RDF [
    <!ENTITY fibo-fnd-plc-adr "http://spec.edmcouncil.org/fibo/red/fnd/places/addresses/">
    <!ENTITY fibo-uo-lat "http://spec.edmcouncil.org/fibo/red/uo/lattice/">
    <!ENTITY fibo-uo-rl "http://spec.edmcouncil.org/fibo/red/uo/relatives/">
    <!ENTITY fibo-rl-set "http://spec.edmcouncil.org/fibo/red/fnd/relative/set-membership/">
    <!ENTITY fibo-fnd-rel-rel "http://spec.edmcouncil.org/fibo/red/fnd/relations/relations/">
    <!ENTITY fibo-fnd-info-info "http://spec.edmcouncil.org/fibo/red/fnd/information/info-core/">
    <!ENTITY fibo-fnd-plc-loc "http://spec.edmcouncil.org/fibo/red/fnd/places/locations/">
    <!ENTITY fibo-fnd-utl-bt "http://spec.edmcouncil.org/fibo/red/fnd/utilities/business-facing-types/">
    <!ENTITY fibo-fnd-plcx-gph "http://spec.edmcouncil.org/fibo/red/fnd/places-ext/geophysical/">
]>

<rdf:RDF xmlns:xsd="http://www.w3.org/2001/XMLSchema#"
         xmlns:sm="http://www.omg.org/techprocess/ab/SpecificationMetadata/"
         xmlns:xs="http://www.w3.org/2001/XMLSchema"
         xmlns:fibo-fnd-utl-av="http://www.omg.org/spec/EDMC-FIBO/FND/Utilities/AnnotationVocabulary/"
         xmlns:rdf="http://www.w3.org/1999/02/22-rdf-syntax-ns#"
         xmlns:rdfs="http://www.w3.org/2000/01/rdf-schema#"
         xmlns:owl="http://www.w3.org/2002/07/owl#"
         xmlns:skos="http://www.w3.org/2004/02/skos/core#"
         xmlns:dc="http://purl.org/dc/terms/"
         xml:base="http://spec.edmcouncil.org/fibo/red/fnd/places/addresses/">

   <owl:Ontology rdf:about="http://spec.edmcouncil.org/fibo/red/fnd/places/addresses/">
      <owl:imports rdf:resource="http://spec.edmcouncil.org/fibo/red/uo/lattice/"/>
      <owl:imports rdf:resource="http://spec.edmcouncil.org/fibo/red/uo/relatives/"/>
      <owl:imports rdf:resource="http://spec.edmcouncil.org/fibo/red/fnd/relative/set-membership/"/>
      <owl:imports rdf:resource="http://spec.edmcouncil.org/fibo/red/fnd/relations/relations/"/>
      <owl:imports rdf:resource="http://spec.edmcouncil.org/fibo/red/fnd/information/info-core/"/>
      <owl:imports rdf:resource="http://spec.edmcouncil.org/fibo/red/fnd/places/locations/"/>
      <owl:imports rdf:resource="http://spec.edmcouncil.org/fibo/red/fnd/utilities/business-facing-types/"/>
      <owl:imports rdf:resource="http://spec.edmcouncil.org/fibo/red/fnd/places-ext/geophysical/"/>
   </owl:Ontology>


  <!--
    ///////////////////////////////////////////////////////////////////////////////////////
    //
    // Datatypes
    //
    ///////////////////////////////////////////////////////////////////////////////////////
    -->



  <!--
    ///////////////////////////////////////////////////////////////////////////////////////
    //
    // Object Properties
    //
    ///////////////////////////////////////////////////////////////////////////////////////
    -->


<owl:ObjectProperty rdf:about="&fibo-fnd-plc-adr;postalAddressIsIndexTo">
      <rdfs:label>postal address is index to</rdfs:label>
      <skos:definition>The place identified by the Address.</skos:definition>
      <rdfs:subPropertyOf rdf:resource="&fibo-fnd-plc-adr;isIndexTo"/>
      <rdfs:domain rdf:resource="&fibo-fnd-plc-adr;PostalAddress"/>
      <rdfs:range rdf:resource="&fibo-fnd-plc-loc;PhysicalLocation"/>
   </owl:ObjectProperty>

   <owl:ObjectProperty rdf:about="&fibo-fnd-plc-adr;stateAbbreviation">
      <rdfs:label>state abbreviation</rdfs:label>
      <skos:definition>Address element giving the formal abbreviation of the state or province (in federal countries) in which the address is situated.</skos:definition>
      <rdfs:subPropertyOf rdf:resource="&fibo-fnd-plc-adr;hasAddressComponent"/>
      <rdfs:domain rdf:resource="&fibo-fnd-plc-adr;Address"/>
      <rdfs:range rdf:resource="&fibo-fnd-plc-adr;AddressComponent"/>
   </owl:ObjectProperty>

   <owl:ObjectProperty rdf:about="&fibo-fnd-plc-adr;hasAddressComponent">
      <rdfs:label>has address component</rdfs:label>
      <skos:definition>The postal address has as part of it some distinct textual element which performs some distinct function within the overall address such as referring to some specific physical place, built property feature or post office box.</skos:definition>
      <rdfs:domain rdf:resource="&fibo-fnd-plc-adr;Address"/>
      <rdfs:range rdf:resource="&fibo-fnd-plc-adr;AddressComponent"/>
   </owl:ObjectProperty>

   <owl:ObjectProperty rdf:about="&fibo-fnd-plc-adr;hasCountryName">
      <rdfs:label>has country name</rdfs:label>
      <skos:definition>The name of the country in which the address is situated, in some format which may be recognized in that or other countries.</skos:definition>
      <rdfs:subPropertyOf rdf:resource="&fibo-fnd-plc-adr;hasAddressComponent"/>
      <rdfs:domain rdf:resource="&fibo-fnd-plc-adr;Address"/>
      <rdfs:range rdf:resource="&fibo-fnd-plc-adr;AddressComponent"/>
   </owl:ObjectProperty>

   <owl:ObjectProperty rdf:about="&fibo-fnd-plc-adr;hasLocality">
      <rdfs:label>has locality</rdfs:label>
      <skos:definition>That part of a written address which uniquely references some town, city or other urban area within the overall address.</skos:definition>
      <rdfs:subPropertyOf rdf:resource="&fibo-fnd-plc-adr;hasAddressComponent"/>
      <rdfs:domain rdf:resource="&fibo-fnd-plc-adr;Address"/>
      <rdfs:range rdf:resource="&fibo-fnd-plc-adr;AddressComponent"/>
   </owl:ObjectProperty>

   <owl:ObjectProperty rdf:about="&fibo-fnd-plc-adr;hasPOBox">
      <rdfs:label>has p o box</rdfs:label>
      <skos:definition>Address element giving the Post Office Box number in the form of digits or letters plus digits.</skos:definition>
      <rdfs:subPropertyOf rdf:resource="&fibo-fnd-plc-adr;hasAddressComponent"/>
      <rdfs:domain rdf:resource="&fibo-fnd-plc-adr;Address"/>
      <rdfs:range rdf:resource="&fibo-fnd-plc-adr;AddressComponent"/>
   </owl:ObjectProperty>

   <owl:ObjectProperty rdf:about="&fibo-fnd-plc-adr;hasPostalCode">
      <rdfs:label>has postal code</rdfs:label>
      <skos:definition>The postal code for an address, in a format recognized by the postal authorities in the country in which the address is situated.</skos:definition>
      <rdfs:subPropertyOf rdf:resource="&fibo-fnd-plc-adr;hasAddressComponent"/>
      <rdfs:domain rdf:resource="&fibo-fnd-plc-adr;Address"/>
      <rdfs:range rdf:resource="&fibo-fnd-plc-adr;AddressComponent"/>
   </owl:ObjectProperty>

   <owl:ObjectProperty rdf:about="&fibo-fnd-plc-adr;hasStateName">
      <rdfs:label>has state name</rdfs:label>
      <skos:definition>Address element giving the name of the state or province (in federal countries) in which the address is situated.</skos:definition>
      <rdfs:subPropertyOf rdf:resource="&fibo-fnd-plc-adr;hasAddressComponent"/>
      <rdfs:domain rdf:resource="&fibo-fnd-plc-adr;Address"/>
      <rdfs:range rdf:resource="&fibo-fnd-plc-adr;AddressComponent"/>
   </owl:ObjectProperty>

   <owl:ObjectProperty rdf:about="&fibo-fnd-plc-adr;hasStreetAddress">
      <rdfs:label>has street address</rdfs:label>
      <skos:definition>Address element giving the building name or number and the street in which the address is situated.</skos:definition>
      <rdfs:subPropertyOf rdf:resource="&fibo-fnd-plc-adr;hasAddressComponent"/>
      <rdfs:domain rdf:resource="&fibo-fnd-plc-adr;Address"/>
      <rdfs:range rdf:resource="&fibo-fnd-plc-adr;AddressComponent"/>
   </owl:ObjectProperty>

   <owl:ObjectProperty rdf:about="&fibo-fnd-plc-adr;isIndexTo">
      <rdfs:label>is index to</rdfs:label>
      <rdfs:subPropertyOf rdf:resource="&fibo-fnd-rel-rel;identifies"/>
      <rdfs:domain rdf:resource="&fibo-fnd-plc-adr;Address"/>
      <rdfs:range rdf:resource="&fibo-fnd-plc-loc;Location"/>
   </owl:ObjectProperty>


  <!--
    ///////////////////////////////////////////////////////////////////////////////////////
    //
    // Data Properties
    //
    ///////////////////////////////////////////////////////////////////////////////////////
    -->


<owl:DatatypeProperty rdf:about="&fibo-fnd-plc-adr;addressElementText">
      <rdfs:label>address element text</rdfs:label>
      <skos:definition>Text which forms part or all of some Address.</skos:definition>
      <rdfs:range rdf:resource="&fibo-fnd-utl-bt;text"/>
   </owl:DatatypeProperty>


  <!--
    ///////////////////////////////////////////////////////////////////////////////////////
    //
    // Annotation Properties
    //
    ///////////////////////////////////////////////////////////////////////////////////////
    -->



  <!--
    ///////////////////////////////////////////////////////////////////////////////////////
    //
    // Classes
    //
    ///////////////////////////////////////////////////////////////////////////////////////
    -->


<owl:Class rdf:about="&fibo-fnd-plc-adr;Address">
      <rdfs:label>address</rdfs:label>
      <skos:definition>An address is an index to a location.</skos:definition>
      <rdfs:subClassOf rdf:resource="&fibo-fnd-info-info;Information"/>
      <rdfs:subClassOf rdf:resource="&fibo-uo-rl;IndependentThing"/>
      <rdfs:subClassOf rdf:resource="&fibo-uo-lat;ContinuantThing"/>
   </owl:Class>

   <owl:Class rdf:about="&fibo-fnd-plc-adr;AddressComponent">
      <rdfs:label>address component</rdfs:label>
      <skos:definition>A textual element which forms part of some Address. Explanatory Note: This textual element may be used in conjunction with other such elements, or it may comprise a hundred percent of the textual content of the address.</skos:definition>
   </owl:Class>

   <owl:Class rdf:about="&fibo-fnd-plc-adr;PostcodeArea">
      <rdfs:label>postcode area</rdfs:label>
      <skos:definition>An area identified specifically by a postal code or part of a postal code.</skos:definition>
      <rdfs:subClassOf rdf:resource="&fibo-fnd-plc-loc;PhysicalLocation"/>
      <rdfs:subClassOf rdf:resource="&fibo-fnd-plcx-gph;GeophysicalLocation"/>
   </owl:Class>

   <owl:Class rdf:about="&fibo-fnd-plc-adr;PostalAddress">
      <rdfs:label>postal address</rdfs:label>
      <skos:definition>A physical and postal address where communications can be addressed, papers served or representatives located for any kind of business entity or legal entity.</skos:definition>
      <rdfs:subClassOf rdf:resource="&fibo-fnd-plc-adr;Address"/>
      <rdfs:subClassOf rdf:resource="&fibo-rl-set;Set"/>
   </owl:Class>


  <!--
    ///////////////////////////////////////////////////////////////////////////////////////
    //
    // Individuals
    //
    ///////////////////////////////////////////////////////////////////////////////////////
    -->


</rdf:RDF>