<?xml version="1.0" encoding="UTF-8"?>
  
<!DOCTYPE rdf:RDF [
    <!ENTITY fibo-fnd-plc-loc "http://spec.edmcouncil.org/fibo/red/fnd/places/locations/">
    <!ENTITY fibo-uo-lat "http://spec.edmcouncil.org/fibo/red/uo/lattice/">
    <!ENTITY fibo-fnd-utl-bt "http://spec.edmcouncil.org/fibo/red/fnd/utilities/business-facing-types/">
    <!ENTITY fibo-uo-rl "http://spec.edmcouncil.org/fibo/red/uo/relatives/">
]>

<rdf:RDF xmlns:xsd="http://www.w3.org/2001/XMLSchema#"
         xmlns:sm="http://www.omg.org/techprocess/ab/SpecificationMetadata/"
         xmlns:xs="http://www.w3.org/2001/XMLSchema"
         xmlns:fibo-fnd-utl-av="http://www.omg.org/spec/EDMC-FIBO/FND/Utilities/AnnotationVocabulary/"
         xmlns:rdf="http://www.w3.org/1999/02/22-rdf-syntax-ns#"
         xmlns:rdfs="http://www.w3.org/2000/01/rdf-schema#"
         xmlns:owl="http://www.w3.org/2002/07/owl#"
         xmlns:skos="http://www.w3.org/2004/02/skos/core#"
         xmlns:dc="http://purl.org/dc/terms/"
         xml:base="http://spec.edmcouncil.org/fibo/red/fnd/places/locations/">

   <owl:Ontology rdf:about="http://spec.edmcouncil.org/fibo/red/fnd/places/locations/">
      <owl:imports rdf:resource="http://spec.edmcouncil.org/fibo/red/uo/lattice/"/>
      <owl:imports rdf:resource="http://spec.edmcouncil.org/fibo/red/fnd/utilities/business-facing-types/"/>
      <owl:imports rdf:resource="http://spec.edmcouncil.org/fibo/red/uo/relatives/"/>
   </owl:Ontology>


  <!--
    ///////////////////////////////////////////////////////////////////////////////////////
    //
    // Datatypes
    //
    ///////////////////////////////////////////////////////////////////////////////////////
    -->



  <!--
    ///////////////////////////////////////////////////////////////////////////////////////
    //
    // Object Properties
    //
    ///////////////////////////////////////////////////////////////////////////////////////
    -->



  <!--
    ///////////////////////////////////////////////////////////////////////////////////////
    //
    // Data Properties
    //
    ///////////////////////////////////////////////////////////////////////////////////////
    -->


<owl:DatatypeProperty rdf:about="&fibo-fnd-plc-loc;leasehold">
      <rdfs:label>leasehold</rdfs:label>
      <skos:definition>Typically a leasehold is where the land is not owned by the borrower, rather it is leased from a third party for a term that exceeds the life of the mortgage.</skos:definition>
      <rdfs:range rdf:resource="&fibo-fnd-utl-bt;yesOrNo"/>
   </owl:DatatypeProperty>


  <!--
    ///////////////////////////////////////////////////////////////////////////////////////
    //
    // Annotation Properties
    //
    ///////////////////////////////////////////////////////////////////////////////////////
    -->



  <!--
    ///////////////////////////////////////////////////////////////////////////////////////
    //
    // Classes
    //
    ///////////////////////////////////////////////////////////////////////////////////////
    -->


<owl:Class rdf:about="&fibo-fnd-plc-loc;PhysicalLocation">
      <rdfs:label>physical location</rdfs:label>
      <skos:definition>A location in physical space.</skos:definition>
      <rdfs:subClassOf rdf:resource="&fibo-fnd-plc-loc;Location"/>
      <rdfs:subClassOf rdf:resource="&fibo-uo-lat;Concrete"/>
   </owl:Class>

   <owl:Class rdf:about="&fibo-fnd-plc-loc;RealEstate">
      <rdfs:label>real estate</rdfs:label>
      <skos:definition>Land plus anything permanently fixed to it, including buildings, sheds and other items attached to the structure. Explanatory Note: Although, media often refers to the "real estate market" from the perspective of residential living, real estate can be grouped into three broad categories based on its use, namely residential, commercial and industrial. Explanatory Note: Examples of real estate include undeveloped land, houses, condominiums, townhomes, office buildings, retail store buildings and factories. Scope Note: Bricks and mortar or land which can be owned.</skos:definition>
      <rdfs:subClassOf rdf:resource="&fibo-fnd-plc-loc;PhysicalLocation"/>
   </owl:Class>

   <owl:Class rdf:about="&fibo-fnd-plc-loc;Location">
      <rdfs:label>location</rdfs:label>
      <skos:definition>Anything that can be defined as the answer to a question of the form "Where is...?"</skos:definition>
      <rdfs:subClassOf rdf:resource="&fibo-uo-rl;IndependentThing"/>
      <rdfs:subClassOf rdf:resource="&fibo-uo-lat;ContinuantThing"/>
   </owl:Class>


  <!--
    ///////////////////////////////////////////////////////////////////////////////////////
    //
    // Individuals
    //
    ///////////////////////////////////////////////////////////////////////////////////////
    -->


</rdf:RDF>