<?xml version="1.0" encoding="UTF-8"?>
  
<!DOCTYPE rdf:RDF [
    <!ENTITY fibo-md-dbt-alx "http://spec.edmcouncil.org/fibo/red/md/debt-temporal/debt-analytics/">
    <!ENTITY fibo-fnd-info-tem "http://spec.edmcouncil.org/fibo/red/fnd/information/temporal-info/">
    <!ENTITY fibo-md-tmp-tmp "http://spec.edmcouncil.org/fibo/red/md/temporal-core/temporal-concepts/">
    <!ENTITY fibo-md-tmp-ins "http://spec.edmcouncil.org/fibo/red/md/temporal-core/instrument-temporal-terms/">
    <!ENTITY fibo-md-dbt-py "http://spec.edmcouncil.org/fibo/red/md/debt-temporal/debt-pricing-yields/">
    <!ENTITY fibo-fnd-tim-tim "http://spec.edmcouncil.org/fibo/red/fnd/date-time/date-time/">
    <!ENTITY fibo-fnd-utl-bt "http://spec.edmcouncil.org/fibo/red/fnd/utilities/business-facing-types/">
    <!ENTITY fibo-fnd-info-info "http://spec.edmcouncil.org/fibo/red/fnd/information/info-core/">
    <!ENTITY fibo-sec-dbt-bond-bond "http://spec.edmcouncil.org/fibo/red/sec/debt/bonds/bonds-common/">
    <!ENTITY fibo-sec-sec-pls "http://spec.edmcouncil.org/fibo/red/sec/securities/pools/">
    <!ENTITY fibo-sec-dbt-ab-pbs "http://spec.edmcouncil.org/fibo/red/sec/debt/asset-backed/pool-backed-securities/">
    <!ENTITY fibo-sec-dbt-ab-abs "http://spec.edmcouncil.org/fibo/red/sec/debt/asset-backed/asset-backed-securities/">
    <!ENTITY fibo-sec-dbt-ab-mbs "http://spec.edmcouncil.org/fibo/red/sec/debt/asset-backed/mortgage-backed-securities/">
    <!ENTITY fibo-uo-rl "http://spec.edmcouncil.org/fibo/red/uo/relatives/">
    <!ENTITY fibo-sec-dbt-dbt-ins "http://spec.edmcouncil.org/fibo/red/sec/debt/debt-foundations/debt-instruments/">
]>

<rdf:RDF xmlns:xsd="http://www.w3.org/2001/XMLSchema#"
         xmlns:sm="http://www.omg.org/techprocess/ab/SpecificationMetadata/"
         xmlns:xs="http://www.w3.org/2001/XMLSchema"
         xmlns:fibo-fnd-utl-av="http://www.omg.org/spec/EDMC-FIBO/FND/Utilities/AnnotationVocabulary/"
         xmlns:rdf="http://www.w3.org/1999/02/22-rdf-syntax-ns#"
         xmlns:rdfs="http://www.w3.org/2000/01/rdf-schema#"
         xmlns:owl="http://www.w3.org/2002/07/owl#"
         xmlns:skos="http://www.w3.org/2004/02/skos/core#"
         xmlns:dc="http://purl.org/dc/terms/"
         xml:base="http://spec.edmcouncil.org/fibo/red/md/debt-temporal/debt-analytics/">

   <owl:Ontology rdf:about="http://spec.edmcouncil.org/fibo/red/md/debt-temporal/debt-analytics/">
      <owl:imports rdf:resource="http://spec.edmcouncil.org/fibo/red/fnd/information/temporal-info/"/>
      <owl:imports rdf:resource="http://spec.edmcouncil.org/fibo/red/md/temporal-core/temporal-concepts/"/>
      <owl:imports rdf:resource="http://spec.edmcouncil.org/fibo/red/md/temporal-core/instrument-temporal-terms/"/>
      <owl:imports rdf:resource="http://spec.edmcouncil.org/fibo/red/md/debt-temporal/debt-pricing-yields/"/>
      <owl:imports rdf:resource="http://spec.edmcouncil.org/fibo/red/fnd/date-time/date-time/"/>
      <owl:imports rdf:resource="http://spec.edmcouncil.org/fibo/red/fnd/utilities/business-facing-types/"/>
      <owl:imports rdf:resource="http://spec.edmcouncil.org/fibo/red/fnd/information/info-core/"/>
      <owl:imports rdf:resource="http://spec.edmcouncil.org/fibo/red/sec/debt/bonds/bonds-common/"/>
      <owl:imports rdf:resource="http://spec.edmcouncil.org/fibo/red/sec/securities/pools/"/>
      <owl:imports rdf:resource="http://spec.edmcouncil.org/fibo/red/sec/debt/asset-backed/pool-backed-securities/"/>
      <owl:imports rdf:resource="http://spec.edmcouncil.org/fibo/red/sec/debt/asset-backed/asset-backed-securities/"/>
      <owl:imports rdf:resource="http://spec.edmcouncil.org/fibo/red/sec/debt/asset-backed/mortgage-backed-securities/"/>
      <owl:imports rdf:resource="http://spec.edmcouncil.org/fibo/red/uo/relatives/"/>
      <owl:imports rdf:resource="http://spec.edmcouncil.org/fibo/red/sec/debt/debt-foundations/debt-instruments/"/>
   </owl:Ontology>


  <!--
    ///////////////////////////////////////////////////////////////////////////////////////
    //
    // Datatypes
    //
    ///////////////////////////////////////////////////////////////////////////////////////
    -->



  <!--
    ///////////////////////////////////////////////////////////////////////////////////////
    //
    // Object Properties
    //
    ///////////////////////////////////////////////////////////////////////////////////////
    -->


<owl:ObjectProperty rdf:about="&fibo-md-dbt-alx;averageLifeValue">
      <rdfs:label>average life value</rdfs:label>
      <skos:definition>The value of the Average Life analytic at some time in the past or at the present. For MBS this would be expressed as a month eg 50 months.</skos:definition>
      <rdfs:domain rdf:resource="&fibo-md-dbt-alx;AverageLife"/>
      <rdfs:range rdf:resource="&fibo-md-tmp-tmp;TimedDurationSpecification"/>
   </owl:ObjectProperty>

   <owl:ObjectProperty rdf:about="&fibo-md-dbt-alx;averageLifeValue.1">
      <rdfs:label>average life value</rdfs:label>
      <skos:definition>The value of the Average Life analytic at the time the security was issued.</skos:definition>
      <rdfs:domain rdf:resource="&fibo-md-dbt-alx;AverageLifeAtIssue"/>
      <rdfs:range rdf:resource="&fibo-fnd-tim-tim;DateSpecification"/>
   </owl:ObjectProperty>

   <owl:ObjectProperty rdf:about="&fibo-md-dbt-alx;takesIntoAccount">
      <rdfs:label>takes into account</rdfs:label>
      <rdfs:subPropertyOf rdf:resource="&fibo-fnd-info-tem;makesReferenceTo"/>
      <rdfs:domain rdf:resource="&fibo-md-dbt-alx;AverageLife"/>
      <rdfs:range rdf:resource="&fibo-md-dbt-alx;PrepaymentSpeed"/>
   </owl:ObjectProperty>

   <owl:ObjectProperty rdf:about="&fibo-md-dbt-alx;definedInRelationTo">
      <rdfs:label>defined in relation to</rdfs:label>
      <rdfs:subPropertyOf rdf:resource="&fibo-fnd-info-tem;makesReferenceTo"/>
      <rdfs:domain rdf:resource="&fibo-md-dbt-alx;DebtConvexityAnalytic"/>
      <rdfs:range rdf:resource="&fibo-md-dbt-py;DebtInstrumentYield"/>
   </owl:ObjectProperty>

   <owl:ObjectProperty rdf:about="&fibo-md-dbt-alx;isRateOfChangeOf">
      <rdfs:label>is rate of change of</rdfs:label>
      <rdfs:subPropertyOf rdf:resource="&fibo-fnd-info-tem;analyzes"/>
      <rdfs:domain rdf:resource="&fibo-md-dbt-alx;DebtConvexityAnalytic"/>
      <rdfs:range rdf:resource="&fibo-md-dbt-alx;DurationAnalytic"/>
   </owl:ObjectProperty>

   <owl:ObjectProperty rdf:about="&fibo-md-dbt-alx;isAbout">
      <rdfs:label>is about</rdfs:label>
      <rdfs:subPropertyOf rdf:resource="&fibo-md-tmp-ins;about"/>
      <rdfs:domain rdf:resource="&fibo-md-dbt-alx;DebtInstrumentAnalyticalParameter"/>
      <rdfs:range rdf:resource="&fibo-sec-dbt-dbt-ins;TradableDebtInstrument"/>
   </owl:ObjectProperty>

   <owl:ObjectProperty rdf:about="&fibo-md-dbt-alx;value">
      <rdfs:label>value</rdfs:label>
      <skos:definition>The numeric value of the Convexity.</skos:definition>
      <rdfs:domain rdf:resource="&fibo-md-dbt-alx;DebtConvexityAnalytic"/>
      <rdfs:range rdf:resource="&fibo-md-tmp-tmp;TimedNumericAmount"/>
   </owl:ObjectProperty>

   <owl:ObjectProperty rdf:about="&fibo-md-dbt-alx;has">
      <rdfs:label>has</rdfs:label>
      <rdfs:subPropertyOf rdf:resource="&fibo-md-dbt-alx;has.1"/>
      <rdfs:domain rdf:resource="&fibo-sec-sec-pls;DebtInstrumentPool"/>
      <rdfs:range rdf:resource="&fibo-md-dbt-alx;DebtInstrumentPoolAnalytic"/>
   </owl:ObjectProperty>

   <owl:ObjectProperty rdf:about="&fibo-md-dbt-alx;hasAnalyticsDetails">
      <rdfs:label>has analytics details</rdfs:label>
      <rdfs:subPropertyOf rdf:resource="&fibo-md-tmp-ins;hasAnalyticsDetails"/>
      <rdfs:domain rdf:resource="&fibo-sec-dbt-dbt-ins;TradableDebtInstrument"/>
      <rdfs:range rdf:resource="&fibo-md-dbt-alx;DebtInstrumentAnalyticalParameter"/>
   </owl:ObjectProperty>

   <owl:ObjectProperty rdf:about="&fibo-md-dbt-alx;has.1">
      <rdfs:label>has</rdfs:label>
      <rdfs:subPropertyOf rdf:resource="&fibo-fnd-info-info;details"/>
      <rdfs:domain rdf:resource="&fibo-sec-sec-pls;DebtPool"/>
      <rdfs:range rdf:resource="&fibo-md-dbt-alx;DebtPoolAnalyticalParameter"/>
   </owl:ObjectProperty>

   <owl:ObjectProperty rdf:about="&fibo-md-dbt-alx;hasFactor">
      <rdfs:label>has factor</rdfs:label>
      <rdfs:domain rdf:resource="&fibo-sec-sec-pls;DebtPool"/>
      <rdfs:range rdf:resource="&fibo-md-dbt-alx;PoolFactor"/>
   </owl:ObjectProperty>

   <owl:ObjectProperty rdf:about="&fibo-md-dbt-alx;refersTo">
      <rdfs:label>refers to</rdfs:label>
      <rdfs:subPropertyOf rdf:resource="&fibo-fnd-info-tem;analyzes"/>
      <rdfs:domain rdf:resource="&fibo-md-dbt-alx;DurationAnalytic"/>
      <rdfs:range rdf:resource="&fibo-md-dbt-py;DebtInstrumentYield"/>
   </owl:ObjectProperty>

   <owl:ObjectProperty rdf:about="&fibo-md-dbt-alx;equivalentLifeValue">
      <rdfs:label>equivalent life value</rdfs:label>
      <skos:definition>The Equivalent Life in years at the stated date.</skos:definition>
      <rdfs:domain rdf:resource="&fibo-md-dbt-alx;EquivalentLifeAnalytic"/>
      <rdfs:range rdf:resource="&fibo-md-tmp-tmp;TimedDurationSpecification"/>
   </owl:ObjectProperty>

   <owl:ObjectProperty rdf:about="&fibo-md-dbt-alx;refersTo.1">
      <rdfs:label>refers to</rdfs:label>
      <rdfs:domain rdf:resource="&fibo-md-dbt-alx;EquivalentLifeAnalytic"/>
      <rdfs:range rdf:resource="&fibo-sec-dbt-bond-bond;BondWithPartialCall"/>
   </owl:ObjectProperty>

   <owl:ObjectProperty rdf:about="&fibo-md-dbt-alx;derivedUsing">
      <rdfs:label>derived using</rdfs:label>
      <rdfs:subPropertyOf rdf:resource="&fibo-fnd-info-tem;derivedFrom"/>
      <rdfs:domain rdf:resource="&fibo-md-dbt-alx;EquivalentLifeAnalytic"/>
      <rdfs:range rdf:resource="&fibo-md-dbt-alx;PartialCallsEstimationModel"/>
   </owl:ObjectProperty>

   <owl:ObjectProperty rdf:about="&fibo-md-dbt-alx;isDefaultIn">
      <rdfs:label>is default in</rdfs:label>
      <rdfs:subPropertyOf rdf:resource="&fibo-uo-rl;inContext"/>
      <rdfs:domain rdf:resource="&fibo-md-dbt-alx;EquivalentYieldCalculationMethod"/>
      <rdfs:range rdf:resource="&fibo-md-dbt-py;BondMarket"/>
   </owl:ObjectProperty>

   <owl:ObjectProperty rdf:about="&fibo-md-dbt-alx;isAggregateOf">
      <rdfs:label>is aggregate of</rdfs:label>
      <rdfs:domain rdf:resource="&fibo-md-dbt-alx;InstrumentAggregateLoanAnalytic"/>
      <rdfs:range rdf:resource="&fibo-md-dbt-py;LoanPoolAnalytic"/>
   </owl:ObjectProperty>

   <owl:ObjectProperty rdf:about="&fibo-md-dbt-alx;aggregateOf">
      <rdfs:label>aggregate of</rdfs:label>
      <rdfs:subPropertyOf rdf:resource="&fibo-md-dbt-alx;isAggregateOf"/>
      <rdfs:domain rdf:resource="&fibo-md-dbt-alx;InstrumentWeightedAverageLoanAge"/>
      <rdfs:range rdf:resource="&fibo-md-dbt-alx;PoolWeightedAverageLoanAge"/>
   </owl:ObjectProperty>

   <owl:ObjectProperty rdf:about="&fibo-md-dbt-alx;aggregateOf.1">
      <rdfs:label>aggregate of</rdfs:label>
      <rdfs:subPropertyOf rdf:resource="&fibo-md-dbt-alx;isAggregateOf"/>
      <rdfs:domain rdf:resource="&fibo-md-dbt-alx;InstrumentWeightedAverageRemainingMaturity"/>
      <rdfs:range rdf:resource="&fibo-md-dbt-alx;PoolWeightedAverageRemainingMaturity"/>
   </owl:ObjectProperty>

   <owl:ObjectProperty rdf:about="&fibo-md-dbt-alx;wALAValue">
      <rdfs:label>w a l a value</rdfs:label>
      <skos:definition>The weighted average loan age, at some point in the past or present.</skos:definition>
      <rdfs:domain rdf:resource="&fibo-md-dbt-alx;InstrumentWeightedAverageLoanAge"/>
      <rdfs:range rdf:resource="&fibo-md-tmp-tmp;TimedDurationSpecification"/>
   </owl:ObjectProperty>

   <owl:ObjectProperty rdf:about="&fibo-md-dbt-alx;value.1">
      <rdfs:label>value</rdfs:label>
      <skos:definition>The value of the IRR at a given point in time, expressed as a percentage.</skos:definition>
      <rdfs:domain rdf:resource="&fibo-md-dbt-alx;InternalRateOfReturn"/>
      <rdfs:range rdf:resource="&fibo-md-tmp-tmp;TimedPercentage"/>
   </owl:ObjectProperty>

   <owl:ObjectProperty rdf:about="&fibo-md-dbt-alx;hasMeasure">
      <rdfs:label>has measure</rdfs:label>
      <rdfs:subPropertyOf rdf:resource="&fibo-md-dbt-py;has.6"/>
      <rdfs:domain rdf:resource="&fibo-sec-dbt-ab-abs;LoanPool"/>
      <rdfs:range rdf:resource="&fibo-md-dbt-alx;PrepaymentSpeed"/>
   </owl:ObjectProperty>

   <owl:ObjectProperty rdf:about="&fibo-md-dbt-alx;modifiedDurationValue">
      <rdfs:label>modified duration value</rdfs:label>
      <skos:definition>The Modified Duration in Years.</skos:definition>
      <rdfs:domain rdf:resource="&fibo-md-dbt-alx;ModifiedDurationAnalytic"/>
      <rdfs:range rdf:resource="&fibo-md-tmp-tmp;TimedDurationSpecification"/>
   </owl:ObjectProperty>

   <owl:ObjectProperty rdf:about="&fibo-md-dbt-alx;refersTo.2">
      <rdfs:label>refers to</rdfs:label>
      <rdfs:domain rdf:resource="&fibo-md-dbt-alx;ModifiedDurationAnalytic"/>
      <rdfs:range rdf:resource="&fibo-md-dbt-py;MacCaulaysDurationAnalytic"/>
   </owl:ObjectProperty>

   <owl:ObjectProperty rdf:about="&fibo-md-dbt-alx;wARMValue">
      <rdfs:label>w a r m value</rdfs:label>
      <skos:definition>The amount of the WARM in the past or present.</skos:definition>
      <rdfs:domain rdf:resource="&fibo-md-dbt-alx;MortgageInstrumentWeightedAverageRemainingMaturity"/>
      <rdfs:range rdf:resource="&fibo-md-tmp-tmp;TimedDurationSpecification"/>
   </owl:ObjectProperty>

   <owl:ObjectProperty rdf:about="&fibo-md-dbt-alx;has.2">
      <rdfs:label>has</rdfs:label>
      <rdfs:subPropertyOf rdf:resource="&fibo-md-dbt-py;has.6"/>
      <rdfs:domain rdf:resource="&fibo-sec-dbt-ab-mbs;MortgagePool"/>
      <rdfs:range rdf:resource="&fibo-md-dbt-alx;PoolWeightedAverageLoanAge"/>
   </owl:ObjectProperty>

   <owl:ObjectProperty rdf:about="&fibo-md-dbt-alx;has.3">
      <rdfs:label>has</rdfs:label>
      <rdfs:subPropertyOf rdf:resource="&fibo-md-dbt-py;has.6"/>
      <rdfs:domain rdf:resource="&fibo-sec-dbt-ab-mbs;MortgagePool"/>
      <rdfs:range rdf:resource="&fibo-md-dbt-alx;PoolWeightedAverageRemainingMaturity"/>
   </owl:ObjectProperty>

   <owl:ObjectProperty rdf:about="&fibo-md-dbt-alx;value.2">
      <rdfs:label>value</rdfs:label>
      <skos:definition>The value of the PVBP expressed as a price change, with price denominated in percentage.</skos:definition>
      <rdfs:domain rdf:resource="&fibo-md-dbt-alx;PVBP"/>
      <rdfs:range rdf:resource="&fibo-md-tmp-tmp;TimedPercentage"/>
   </owl:ObjectProperty>

   <owl:ObjectProperty rdf:about="&fibo-md-dbt-alx;definedInRelationTo.1">
      <rdfs:label>defined in relation to</rdfs:label>
      <rdfs:subPropertyOf rdf:resource="&fibo-fnd-info-tem;makesReferenceTo"/>
      <rdfs:domain rdf:resource="&fibo-md-dbt-alx;PVBP"/>
      <rdfs:range rdf:resource="&fibo-md-dbt-py;DebtInstrumentYield"/>
   </owl:ObjectProperty>

   <owl:ObjectProperty rdf:about="&fibo-md-dbt-alx;has.4">
      <rdfs:label>has</rdfs:label>
      <rdfs:domain rdf:resource="&fibo-sec-dbt-ab-pbs;PoolBackedSecurityInstrument"/>
      <rdfs:range rdf:resource="&fibo-md-dbt-alx;InstrumentWeightedAverageRemainingMaturity"/>
   </owl:ObjectProperty>

   <owl:ObjectProperty rdf:about="&fibo-md-dbt-alx;factorValue">
      <rdfs:label>factor value</rdfs:label>
      <skos:definition>The factor, expressed as a numberic amount in the past or present.</skos:definition>
      <rdfs:domain rdf:resource="&fibo-md-dbt-alx;PoolFactor"/>
      <rdfs:range rdf:resource="&fibo-md-tmp-tmp;TimedPercentage"/>
   </owl:ObjectProperty>

   <owl:ObjectProperty rdf:about="&fibo-md-dbt-alx;prepaymentSpeedValue">
      <rdfs:label>prepayment speed value</rdfs:label>
      <rdfs:domain rdf:resource="&fibo-md-dbt-alx;PrepaymentSpeed"/>
      <rdfs:range rdf:resource="&fibo-md-tmp-tmp;DatedPercentage"/>
   </owl:ObjectProperty>

   <owl:ObjectProperty rdf:about="&fibo-md-dbt-alx;determinedBy">
      <rdfs:label>determined by</rdfs:label>
      <rdfs:subPropertyOf rdf:resource="&fibo-fnd-info-tem;derivedFrom"/>
      <rdfs:domain rdf:resource="&fibo-md-dbt-alx;PrepaymentSpeed"/>
      <rdfs:range rdf:resource="&fibo-md-dbt-py;LoanPoolPrepaymentModel"/>
   </owl:ObjectProperty>


  <!--
    ///////////////////////////////////////////////////////////////////////////////////////
    //
    // Data Properties
    //
    ///////////////////////////////////////////////////////////////////////////////////////
    -->


<owl:DatatypeProperty rdf:about="&fibo-md-dbt-alx;averageLifeDateAtIssue">
      <rdfs:label>average life date at issue</rdfs:label>
      <skos:definition>The date equivalent to the Average Life figure, as measured at Issue Date.</skos:definition>
      <rdfs:range rdf:resource="http://www.w3.org/2001/XMLSchema#date"/>
   </owl:DatatypeProperty>

   <owl:DatatypeProperty rdf:about="&fibo-md-dbt-alx;decimalPlaces">
      <rdfs:label>decimal places</rdfs:label>
      <skos:definition>The number of decimal places used in the publication of the factor value.</skos:definition>
      <rdfs:range rdf:resource="&fibo-fnd-utl-bt;wholeNumber"/>
   </owl:DatatypeProperty>


  <!--
    ///////////////////////////////////////////////////////////////////////////////////////
    //
    // Annotation Properties
    //
    ///////////////////////////////////////////////////////////////////////////////////////
    -->



  <!--
    ///////////////////////////////////////////////////////////////////////////////////////
    //
    // Classes
    //
    ///////////////////////////////////////////////////////////////////////////////////////
    -->


<owl:Class rdf:about="&fibo-md-dbt-alx;AverageLife">
      <rdfs:label>average life</rdfs:label>
      <skos:definition>An estimate of the number of terms to maturity, taking the possibility of early payments into account. Average life is calculated using the weighted average time to the receipt of all future cash flows.</skos:definition>
      <rdfs:subClassOf rdf:resource="&fibo-md-dbt-alx;LifeAnalytic"/>
   </owl:Class>

   <owl:Class rdf:about="&fibo-md-dbt-alx;AverageLifeAtIssue">
      <rdfs:label>average life at issue</rdfs:label>
      <skos:definition>The Average Life analytic at the time the security was issued.</skos:definition>
      <rdfs:subClassOf rdf:resource="&fibo-md-dbt-alx;AverageLife"/>
   </owl:Class>

   <owl:Class rdf:about="&fibo-md-dbt-alx;DebtConvexityAnalytic">
      <rdfs:label>debt convexity analytic</rdfs:label>
      <skos:definition>The second derivative of a security's price with respect to its yield, divided by the security's price. A security exhibits positive convexity when its price rises more for a downward move in its yield than its price declines for an equal upward move in its yield. Further notes: A measure of the change in price for a given change in Modified Duration. This always (necessarily) refers to Modified Duration. This is used as another risk measurement. Numerator is always (a) duration - either MacCaulays or Modified. Always rate of change of (one of the) Duration against some other parameter. The other paramater can be characterised as a Yield (it may be the Price, but that has a relationship to the Yield in any case). REVIEW: Inconsistency in the above - is it always necessarily Modified Duration that is referred to, or "any" Duration measure (Macaulays and.or Modified)? notes 9 Dec A measure of the sensitivity of the price with reference to interest rates. This is normally determined with reference to maturity, but since there are different maturity dates, this figure gives an estimate of the equitvalent if you had a homogenous portfolio, i.e. this is an estimate based on a pure equivalent, homogenous portfolio. Convexity of instrument versus portfolio. Sees instrument in terms of the set of cashflows. The term Convexity can be applied either to a bond or to a portfolio. More notes: When you get Convexit in MD, it will tell you what Duration it is refrfering to, along with Redemption Date (logically). Also if there is Option Adjusted Yield, there is a third set of analytics. What are they? i.e. OA Convexity, Duration Yield and the rest. Conclusions: Agreed to revisit this in OTC.</skos:definition>
      <rdfs:subClassOf rdf:resource="&fibo-md-tmp-tmp;CurveConvexity"/>
   </owl:Class>

   <owl:Class rdf:about="&fibo-md-dbt-alx;DebtInstrumentAnalyticalParameter">
      <rdfs:label>debt instrument analytical parameter</rdfs:label>
      <skos:definition>Parameter describing some aspect of the behaviour of a debt instrument, that may vary over time.</skos:definition>
      <rdfs:subClassOf rdf:resource="&fibo-md-tmp-ins;FinancialInstrumentAnalyticalParameter"/>
   </owl:Class>

   <owl:Class rdf:about="&fibo-md-dbt-alx;DebtInstrumentPoolAnalytic">
      <rdfs:label>debt instrument pool analytic</rdfs:label>
      <skos:definition>A measure of some aspect of the behaviour or a pool of securitized debt i.e. a pool of debt instruments. Futher Notes: Nothing defined under this yet. We have analytics for pools of individual debt products (mortgages, loans, auto loans), but not the equivalent sorts of terms implied for a securitixed debt pool. Presumably these would be aggregate terms similar or equivalent to analytics for debt instruments, such as yield, average live, convixity and so on. As such these would be similar to porfolio analytics (not modeled).</skos:definition>
      <rdfs:subClassOf rdf:resource="&fibo-md-dbt-alx;DebtPoolAnalyticalParameter"/>
   </owl:Class>

   <owl:Class rdf:about="&fibo-md-dbt-alx;DebtPoolAnalyticalParameter">
      <rdfs:label>debt pool analytical parameter</rdfs:label>
      <skos:definition>A measure of some aspect of some pool of debt, such as a pool of loans or a pool of securitized debt products.</skos:definition>
      <rdfs:subClassOf rdf:resource="&fibo-md-dbt-alx;PoolAnalyticalParameter"/>
   </owl:Class>

   <owl:Class rdf:about="&fibo-md-dbt-alx;DurationAnalytic">
      <rdfs:label>duration analytic</rdfs:label>
      <skos:definition>Weighted average time to receipt of all the payments.</skos:definition>
      <rdfs:subClassOf rdf:resource="&fibo-md-dbt-alx;DebtInstrumentAnalyticalParameter"/>
   </owl:Class>

   <owl:Class rdf:about="&fibo-md-dbt-alx;EffectiveDuration">
      <rdfs:label>effective duration</rdfs:label>
      <rdfs:subClassOf rdf:resource="&fibo-md-dbt-alx;DurationAnalytic"/>
   </owl:Class>

   <owl:Class rdf:about="&fibo-md-dbt-alx;EquivalentLifeAnalytic">
      <rdfs:label>equivalent life analytic</rdfs:label>
   </owl:Class>

   <owl:Class rdf:about="&fibo-md-dbt-alx;EquivalentYieldCalculationMethod">
      <rdfs:label>equivalent yield calculation method</rdfs:label>
      <rdfs:subClassOf rdf:resource="&fibo-md-dbt-py;RelativeYieldCalculationMethod"/>
   </owl:Class>

   <owl:Class rdf:about="&fibo-md-dbt-alx;FFIECDown300PrepaySpeed">
      <rdfs:label>f f i e c down 300 prepay speed</rdfs:label>
      <skos:definition>Public Securities Association (PSA) speed used for the underlying collateral for cash-flow calculations in the "down 300" scenario.</skos:definition>
      <rdfs:subClassOf rdf:resource="&fibo-md-dbt-alx;PrepaymentSpeed"/>
   </owl:Class>

   <owl:Class rdf:about="&fibo-md-dbt-alx;FFIECUp300PrepaySpeed">
      <rdfs:label>f f i e c up 300 prepay speed</rdfs:label>
      <skos:definition>Public Securities Association (PSA) speed used for the underlying collateral for cash-flow calculations in the "up 300" scenario.</skos:definition>
   </owl:Class>

   <owl:Class rdf:about="&fibo-md-dbt-alx;ICMAYieldFormula">
      <rdfs:label>i c m a yield formula</rdfs:label>
      <skos:definition>The calculation method specified by ICMA (formerly ISMA) for determination of yield for fixed-rate bonds.</skos:definition>
      <rdfs:subClassOf rdf:resource="&fibo-md-dbt-py;YieldCalculationFormula"/>
   </owl:Class>

   <owl:Class rdf:about="&fibo-md-dbt-alx;ImpliedForwardRate">
      <rdfs:label>implied forward rate</rdfs:label>
   </owl:Class>

   <owl:Class rdf:about="&fibo-md-dbt-alx;InstrumentAggregateLoanAnalytic">
      <rdfs:label>instrument aggregate loan analytic</rdfs:label>
      <skos:definition>Parameters that describe some feature of loan pools or mortgage pools, aggregated and defined at the level of the instrument (i.e. the tranche or class of security within the issue).</skos:definition>
   </owl:Class>

   <owl:Class rdf:about="&fibo-md-dbt-alx;InstrumentInternalRateOfReturn">
      <rdfs:label>instrument internal rate of return</rdfs:label>
      <skos:definition>The discount rate that results in a Net Present Value of zero for a series of future cash flows for the holder of the financial instrument.</skos:definition>
      <rdfs:subClassOf rdf:resource="&fibo-md-dbt-alx;InternalRateOfReturn"/>
   </owl:Class>

   <owl:Class rdf:about="&fibo-md-dbt-alx;InstrumentWeightedAverageLoanAge">
      <rdfs:label>instrument weighted average loan age</rdfs:label>
      <skos:definition>A dollar-weighted average measuring the age of the individual loans in a mortgage pass-through or pooled security, such as Ginnie Mae or a Freddie Mac security. The WALA is measured as the time in months since the origination of the loans, with the weighting based on each loan's size in proportion to the aggregate total of the pool.</skos:definition>
      <rdfs:subClassOf rdf:resource="&fibo-md-dbt-alx;InstrumentAggregateLoanAnalytic"/>
   </owl:Class>

   <owl:Class rdf:about="&fibo-md-dbt-alx;InstrumentWeightedAverageRemainingMaturity">
      <rdfs:label>instrument weighted average remaining maturity</rdfs:label>
      <skos:definition>The weighted average of the time until all maturities on loans in a mortgage-backed or asset backed security. The higher the weighted average to maturity of the loans, the longer the loans in the security have until maturity.</skos:definition>
   </owl:Class>

   <owl:Class rdf:about="&fibo-md-dbt-alx;InternalRateOfReturn">
      <rdfs:label>internal rate of return</rdfs:label>
      <skos:definition>The discount rate that results in a Net Present Value of zero for a series of future cash flows.</skos:definition>
      <rdfs:subClassOf rdf:resource="&fibo-fnd-info-tem;AnalyticalInformation"/>
   </owl:Class>

   <owl:Class rdf:about="&fibo-md-dbt-alx;InternallyDeterminedPriceSpread">
      <rdfs:label>internally determined price spread</rdfs:label>
      <skos:definition>The spread determined internally within the organisation from information available at their own trading desks. Further Notes Internal prices within a bank would be determined by surveying their own traders. So e.g. corporate desk trades these 30 bonds, get the daily spreads on those at the end of the day and calculate the price. The traders determine the pricing during the based on market movements. (this is all for OTC traded bonds, not exchange traded bonds).</skos:definition>
      <rdfs:subClassOf rdf:resource="&fibo-md-dbt-py;DebtPriceSpread"/>
   </owl:Class>

   <owl:Class rdf:about="&fibo-md-dbt-alx;KeyRateDuration">
      <rdfs:label>key rate duration</rdfs:label>
   </owl:Class>

   <owl:Class rdf:about="&fibo-md-dbt-alx;LifeAnalytic">
      <rdfs:label>life analytic</rdfs:label>
      <skos:definition>Some measure of the life of a security, other than the actual time to maturity itself. This is a derived figure, based on certain parameters as appropriate to that type of instrument, to give a figure that is equivalent to and similar to the basic maturity of the instrument, for the purposes of analysing that security.</skos:definition>
   </owl:Class>

   <owl:Class rdf:about="&fibo-md-dbt-alx;MaturityEquivalentPSA">
      <rdfs:label>maturity equivalent p s a</rdfs:label>
      <skos:definition>Prepayment speed that results in the same average life as that computed for the Collateralized Mortgage Obligation (CMO), Asset Backed Securities (ABS) or Mortgage Backed Securities (MBS) using the Maturity Prepay Model.</skos:definition>
   </owl:Class>

   <owl:Class rdf:about="&fibo-md-dbt-alx;ModifiedDurationAnalytic">
      <rdfs:label>modified duration analytic</rdfs:label>
      <skos:definition>The percentage price change of a security for a given change in yield. The higher the modified duration of a security, the higher its risk. Ad/ModDuration = [duration / {1 + (IRR/M)}]; where IRR is the internal rate of return and M is the number of compounding periods per year.</skos:definition>
   </owl:Class>

   <owl:Class rdf:about="&fibo-md-dbt-alx;MortgageInstrumentWeightedAverageRemainingMaturity">
      <rdfs:label>mortgage instrument weighted average remaining maturity</rdfs:label>
      <skos:definition>The weighted average of the time until all maturities on mortgages in a mortgage-backed security (MBS). The higher the weighted average to maturity, the longer the mortgages in the security have until maturity. Synonym (if this is the same term): Also known as "average effective maturity".</skos:definition>
      <rdfs:subClassOf rdf:resource="&fibo-md-dbt-alx;InstrumentWeightedAverageRemainingMaturity"/>
   </owl:Class>

   <owl:Class rdf:about="&fibo-md-dbt-alx;PVBP">
      <rdfs:label>p v b p</rdfs:label>
      <skos:definition>Sensitivity of the price for one basis point change in yield, defined as the difference in price given 1 bp change in yield.</skos:definition>
   </owl:Class>

   <owl:Class rdf:about="&fibo-md-dbt-alx;PartialCallsEstimationModel">
      <rdfs:label>partial calls estimation model</rdfs:label>
      <skos:definition>A model of how the early partial calls are estimated.</skos:definition>
      <rdfs:subClassOf rdf:resource="&fibo-fnd-info-tem;AnalyticsCalculationModel"/>
   </owl:Class>

   <owl:Class rdf:about="&fibo-md-dbt-alx;PoolAnalyticalParameter">
      <rdfs:label>pool analytical parameter</rdfs:label>
      <skos:definition>Paramater that describes some aspect of the behaviour of some kind of pool.</skos:definition>
   </owl:Class>

   <owl:Class rdf:about="&fibo-md-dbt-alx;PoolFactor">
      <rdfs:label>pool factor</rdfs:label>
      <skos:definition>How much of the original pool is still outstanding. This is a number below one. Expressed as percentage.</skos:definition>
      <rdfs:subClassOf rdf:resource="&fibo-md-tmp-ins;ReferenceFactor"/>
   </owl:Class>

   <owl:Class rdf:about="&fibo-md-dbt-alx;PoolPaydownRate">
      <rdfs:label>pool paydown rate</rdfs:label>
      <skos:definition>The rate at which the pool is paying down. This is based on observed factor. CPR, SMM, etc. etc. Measured differently for different kinds of security. CBO might have a prepayment rate for example if the underlying bond is callable. with a non agency mortgge dela, defualts will effect this. so for instance there is principal is no lnger inthe pool because the mortgagee defaults. With agency these are not taken out in the case of default but for non agency these mortgages are removed from the pool if and when a mortgagee defualts.</skos:definition>
   </owl:Class>

   <owl:Class rdf:about="&fibo-md-dbt-alx;PoolWeightedAverageLoanAge">
      <rdfs:label>pool weighted average loan age</rdfs:label>
      <skos:definition>A dollar-weighted average measuring the age of the individual loans in a mortgage pass-through or pooled security, such as Ginnie Mae or a Freddie Mac security. The WALA is measured as the time in months since the origination of the loans, with the weighting based on each loan's size in proportion to the aggregate total of the pool.</skos:definition>
      <rdfs:subClassOf rdf:resource="&fibo-md-dbt-py;LoanPoolAnalytic"/>
   </owl:Class>

   <owl:Class rdf:about="&fibo-md-dbt-alx;PoolWeightedAverageRemainingMaturity">
      <rdfs:label>pool weighted average remaining maturity</rdfs:label>
      <skos:definition>The weighted average of the time until all maturities on loans in a pool. The higher the weighted average to maturity of the loans, the longer the loans in the pool have until maturity. REVIEW: Adapted from instrument specific definition from Investopedia. Review of 23 September identified that certain figures exist for pool and for instrument, whereas Investopedia definition was for Instrument (tranche, class etc.).</skos:definition>
   </owl:Class>

   <owl:Class rdf:about="&fibo-md-dbt-alx;PrepaymentSpeed">
      <rdfs:label>prepayment speed</rdfs:label>
      <skos:definition>The rate at which the pool is paying down. Further Notes 02 Dec: This is a model. Includes other factors such as homogeniety. Earlier notes: Same as Payment. Curtailment. Paydown is normally scheduled payments of the mortgage. Prepayment is when someone pays off the mortgage early I may send in 1500 when my monthly amount is 1000 a month. So the 500 is a prepayment. Scheduled principal payment. More notes 25 nov: Also factor in changes to the pool constituents where this is allowed for that kind of MBS. So we make estimates of how face value will will change. face value won't change but the underlying value of the Pf changes, so eg. the current mortgage factor. Model update note June 2010: Detailed types of "Prepayment Speed" analytic received from thomson Reuters, now modeled as sub types of this term. So term origin is PSA by extension, since this is the common super class of 3 specific prepayment speed analytic types defined by PSA. PSA stands for Public Securities Association. Type: PSA gives this as numeric, however definitions imply percentage, so defined as dated percentage for now. Many data models use numbers which are interpreted later as percentages so this may be the case here.</skos:definition>
   </owl:Class>

   <owl:Class rdf:about="&fibo-md-dbt-alx;PriceAnalytic">
      <rdfs:label>price analytic</rdfs:label>
      <skos:definition>Information that is about prices, rather than actually being a price.</skos:definition>
      <rdfs:subClassOf rdf:resource="&fibo-md-tmp-ins;MarketData"/>
   </owl:Class>


  <!--
    ///////////////////////////////////////////////////////////////////////////////////////
    //
    // Individuals
    //
    ///////////////////////////////////////////////////////////////////////////////////////
    -->


</rdf:RDF>