<?xml version="1.0" encoding="UTF-8"?>
<rdf:RDF xmlns:xsd="http://www.w3.org/2001/XMLSchema#"
         xmlns:sm="http://www.omg.org/techprocess/ab/SpecificationMetadata/"
         xmlns:fibo-fnd-utl-av="http://www.omg.org/spec/EDMC-FIBO/FND/Utilities/AnnotationVocabulary/"
         xmlns:rdf="http://www.w3.org/1999/02/22-rdf-syntax-ns#"
         xmlns:rdfs="http://www.w3.org/2000/01/rdf-schema#"
         xmlns:owl="http://www.w3.org/2002/07/owl#"
         xmlns:skos="http://www.w3.org/2004/02/skos/core#"
         xmlns:dc="http://purl.org/dc/terms/"
         xml:base="http://www.omg.org/spec/EDMC-SR/FND/Parties/Roles/">

   <owl:Ontology rdf:about="http://www.omg.org/spec/EDMC-SR/FND/Parties/Roles/"/>

   <!--Datatypes-->

<!--Object Properties-->

<owl:ObjectProperty rdf:about="http://www.omg.org/spec/EDMC-SR/FND/Parties/Roles/agentInRoleHasRole">
      <rdfs:subPropertyOf rdf:resource="http://www.omg.org/spec/EDMC-SR/FND/Parties/Roles/hasRole"/>
      <rdfs:domain rdf:resource="http://www.omg.org/spec/EDMC-SR/FND/Parties/Roles/AgentInRole"/>
      <rdfs:range rdf:resource="http://www.omg.org/spec/EDMC-SR/FND/Parties/Roles/Role"/>
   </owl:ObjectProperty>

   <owl:ObjectProperty rdf:about="http://www.omg.org/spec/EDMC-SR/FND/Parties/Roles/agentInroleHasIdentity">
      <skos:definition>The identity of the Independent Thing which is defined as some kind of AgentInRole.</skos:definition>
      <rdfs:subPropertyOf rdf:resource="http://www.omg.org/spec/EDMC-SR/FND/Relations/Relations/hasIdentity"/>
      <rdfs:domain rdf:resource="http://www.omg.org/spec/EDMC-SR/FND/Parties/Roles/AgentInRole"/>
      <rdfs:range rdf:resource="http://www.edmcouncil.org/spec/EDMC-SR/UO/OntologicalDegree/IndependentThing"/>
   </owl:ObjectProperty>

   <owl:ObjectProperty rdf:about="http://www.omg.org/spec/EDMC-SR/FND/Parties/Roles/hasRole">
      <skos:definition>provides a means for relating a person, organization, group, or other entity to a role that entity plays in some relationship and context</skos:definition>
      <rdfs:domain rdf:resource="http://www.omg.org/spec/EDMC-SR/FND/Relations/Relations/Thing"/>
      <rdfs:range rdf:resource="http://www.omg.org/spec/EDMC-SR/FND/Parties/Roles/Role"/>
   </owl:ObjectProperty>

   <!--Data Properties-->

<!--Annotation Properties-->

<!--Classes-->

<owl:Class rdf:about="http://www.omg.org/spec/EDMC-SR/FND/Parties/Roles/AgentInRole">
      <rdfs:label>AgentInRole</rdfs:label>
      <skos:definition>An agent-in-role is a relative concept that ties an autonomous agent to a role they are playing in a given situational context.</skos:definition>
      <rdfs:subClassOf rdf:resource="http://www.edmcouncil.org/spec/EDMC-SR/UO/OntologicalDegree/RelativeThing"/>
   </owl:Class>

   <owl:Class rdf:about="http://www.omg.org/spec/EDMC-SR/FND/Parties/Roles/Role">
      <rdfs:label>Role</rdfs:label>
      <skos:definition>A role is a set of connected behaviours, rights, obligations, beliefs, and norms as conceptualised by actors in the context of some situation.</skos:definition>
   </owl:Class>

   <!--Individuals-->

</rdf:RDF>