<?xml version="1.0" encoding="UTF-8"?>
<rdf:RDF xmlns:xsd="http://www.w3.org/2001/XMLSchema#"
         xmlns:sm="http://www.omg.org/techprocess/ab/SpecificationMetadata/"
         xmlns:fibo-fnd-utl-av="http://www.omg.org/spec/EDMC-FIBO/FND/Utilities/AnnotationVocabulary/"
         xmlns:rdf="http://www.w3.org/1999/02/22-rdf-syntax-ns#"
         xmlns:rdfs="http://www.w3.org/2000/01/rdf-schema#"
         xmlns:owl="http://www.w3.org/2002/07/owl#"
         xmlns:skos="http://www.w3.org/2004/02/skos/core#"
         xmlns:dc="http://purl.org/dc/terms/"
         xml:base="http://www.omg.org/spec/EDMC-SR/BE/LegalEntities/LegalPersons/">

   <owl:Ontology rdf:about="http://www.omg.org/spec/EDMC-SR/BE/LegalEntities/LegalPersons/">
      <owl:imports rdf:resource="http://www.omg.org/spec/EDMC-SR/FND/Accounting/CurrencyAmount/"/>
      <owl:imports rdf:resource="http://www.omg.org/spec/EDMC-SR/BE/LegalEntities/FormalBusinessOrganizations/"/>
      <owl:imports rdf:resource="http://www.omg.org/spec/EDMC-SR/FND/Law/Jurisdictions/"/>
      <owl:imports rdf:resource="http://www.omg.org/spec/EDMC-SR/FND/Law/LegalCapacities/"/>
      <owl:imports rdf:resource="http://www.omg.org/spec/EDMC-SR/FND/Law/LegalCore/"/>
   </owl:Ontology>

   <!--Datatypes-->

<!--Object Properties-->

<owl:ObjectProperty rdf:about="http://www.omg.org/spec/EDMC-SR/BE/LegalEntities/LegalPersons/legalPersonHasCapacity">
      <rdfs:subPropertyOf rdf:resource="http://www.omg.org/spec/EDMC-SR/FND/Law/LegalCapacities/hasCapacity"/>
      <rdfs:domain rdf:resource="http://www.omg.org/spec/EDMC-SR/BE/LegalEntities/LegalPersons/LegalPerson"/>
      <rdfs:range rdf:resource="http://www.omg.org/spec/EDMC-SR/FND/Law/LegalCapacities/LiabilityCapacity"/>
      <owl:inverseOf rdf:resource="http://www.edmcouncil.org/spec/EDMC-SR/BE/LegalEntitiesExt/LegalPersonsExtended/accruesTo"/>
   </owl:ObjectProperty>

   <owl:ObjectProperty rdf:about="http://www.omg.org/spec/EDMC-SR/BE/LegalEntities/LegalPersons/powerO.fAttorneyIsConferredOn">
      <rdfs:subPropertyOf rdf:resource="http://www.omg.org/spec/EDMC-SR/FND/Law/LegalCapacities/legalConstructIsConferredOn"/>
      <rdfs:domain rdf:resource="http://www.omg.org/spec/EDMC-SR/BE/LegalEntities/LegalPersons/PowerOfAttorney"/>
      <rdfs:range rdf:resource="http://www.omg.org/spec/EDMC-SR/BE/LegalEntities/LegalPersons/NaturalPerson"/>
   </owl:ObjectProperty>

   <owl:ObjectProperty rdf:about="http://www.omg.org/spec/EDMC-SR/BE/LegalEntities/LegalPersons/hasCapacity">
      <skos:definition>Has the capacity to sign contracts on behalf of some entity.</skos:definition>
      <rdfs:subPropertyOf rdf:resource="http://www.omg.org/spec/EDMC-SR/FND/Law/LegalCapacities/hasCapacity"/>
      <rdfs:domain rdf:resource="http://www.omg.org/spec/EDMC-SR/BE/LegalEntities/LegalPersons/Signatory"/>
      <rdfs:range rdf:resource="http://www.omg.org/spec/EDMC-SR/FND/Law/LegalCapacities/SignatoryCapacity"/>
   </owl:ObjectProperty>

   <owl:ObjectProperty rdf:about="http://www.omg.org/spec/EDMC-SR/BE/LegalEntities/LegalPersons/signatoryHasIdentity">
      <skos:definition>The identity of the Signatory. This has to be some natural person (some human being who has legal capacity).</skos:definition>
      <rdfs:subPropertyOf rdf:resource="http://www.omg.org/spec/EDMC-SR/FND/Parties/Parties/partyInRoleHasIdentity"/>
      <rdfs:domain rdf:resource="http://www.omg.org/spec/EDMC-SR/BE/LegalEntities/LegalPersons/Signatory"/>
      <rdfs:range rdf:resource="http://www.omg.org/spec/EDMC-SR/BE/LegalEntities/LegalPersons/NaturalPerson"/>
   </owl:ObjectProperty>

   <owl:ObjectProperty rdf:about="http://www.omg.org/spec/EDMC-SR/BE/LegalEntities/LegalPersons/designatesSignatory">
      <skos:definition>Designates a party able to sign contracts on the part of the Legal Person.</skos:definition>
      <rdfs:subPropertyOf rdf:resource="http://www.omg.org/spec/EDMC-SR/FND/Relations/Relations/designates"/>
      <rdfs:subPropertyOf rdf:resource="http://www.omg.org/spec/EDMC-SR/FND/Parties/Parties/hasPartyInRole"/>
      <rdfs:domain rdf:resource="http://www.omg.org/spec/EDMC-SR/BE/LegalEntities/LegalPersons/LegalPerson"/>
      <rdfs:range rdf:resource="http://www.omg.org/spec/EDMC-SR/BE/LegalEntities/LegalPersons/Signatory"/>
   </owl:ObjectProperty>

   <owl:ObjectProperty rdf:about="http://www.omg.org/spec/EDMC-SR/BE/LegalEntities/LegalPersons/tradingAtPostalAddress">
      <skos:definition>Address at which the Body Corporate carries out its business.</skos:definition>
      <rdfs:subPropertyOf rdf:resource="http://www.omg.org/spec/EDMC-SR/BE/LegalEntities/FormalBusinessOrganizations/hasOperatingAddress"/>
      <rdfs:domain rdf:resource="http://www.omg.org/spec/EDMC-SR/BE/LegalEntities/CorporateBodies/BodyCorporate"/>
      <rdfs:range rdf:resource="http://www.omg.org/spec/EDMC-SR/FND/Places/Addresses/PostalAddress"/>
   </owl:ObjectProperty>

   <!--Data Properties-->

<!--Annotation Properties-->

<!--Classes-->

<owl:Class rdf:about="http://www.omg.org/spec/EDMC-SR/BE/LegalEntities/LegalPersons/CharteredLegalPerson">
      <rdfs:label>Chartered Legal Person</rdfs:label>
      <skos:definition>A Legal Person created by some Royal Charter or Decree.</skos:definition>
      <skos:editorialNote>Would only exist in a monarchy or principality, The monarch typically vests the power to create such bodies, in an entity called (for example) the Privy Council. Editorial Note: In general, companies / entities may be created by Act of Parliament or by Royal Charter. Royal Charter is created by the Privy Council rather than by Parliament. This would not exist in a republic. Examples: Anything with "Royal Institute" in the name. Also University generally set up by royal charter (often pre-dating any Privy Council i.e. directly be the monarch in the case of older universities). The Bank of England and the British Broadcasting Council (BBC) are also incorporated through Royal Charter. Editorial Note: Control - possibly vested in the Privy Council unless this is only the power to set up (or to dissolve?) Further research required.</skos:editorialNote>
      <rdfs:subClassOf rdf:resource="http://www.omg.org/spec/EDMC-SR/BE/LegalEntities/LegalPersons/JudicialPerson"/>
   </owl:Class>

   <owl:Class rdf:about="http://www.omg.org/spec/EDMC-SR/BE/LegalEntities/LegalPersons/JudicialPerson">
      <rdfs:label>Judicial Person</rdfs:label>
      <rdfs:subClassOf rdf:resource="http://www.omg.org/spec/EDMC-SR/BE/LegalEntities/LegalPersons/LegalPerson"/>
   </owl:Class>

   <owl:Class rdf:about="http://www.omg.org/spec/EDMC-SR/BE/LegalEntities/LegalPersons/LegalPerson">
      <rdfs:label>Legal Person</rdfs:label>
      <rdfs:subClassOf rdf:resource="http://www.omg.org/spec/EDMC-SR/FND/AgentsAndPeople/Agents/AutonomousAgent"/>
   </owl:Class>

   <owl:Class rdf:about="http://www.omg.org/spec/EDMC-SR/BE/LegalEntities/LegalPersons/PowerOfAttorney">
      <rdfs:label>Power Of Attorney</rdfs:label>
      <skos:definition>Written legal authority given by one party (the principal) to another (the agent or attorney-in-fact) to act on the principals behalf. It may be a (1) General power Of attorney that authorizes the agent to act generally on behalf of the principal, or (2) Special power of attorney that is limited to a specific act or situation. Decisions made and actions taken by an attorney in fact (within the scope of his or her authority) are legally binding on the principal. A power of attorney can remain in force only so long as the principal is alive and does not become disabled or incapacitated. Although it is often conferred on the principals attorney, one does not need to be an attorney at law to be an attorney-in-fact.</skos:definition>
      <rdfs:subClassOf rdf:resource="http://www.omg.org/spec/EDMC-SR/FND/Law/LegalCapacities/LegalCapacity"/>
   </owl:Class>

   <owl:Class rdf:about="http://www.omg.org/spec/EDMC-SR/BE/LegalEntities/LegalPersons/Signatory">
      <rdfs:label>Signatory</rdfs:label>
      <skos:definition>Some agent who has the capacity to sign contracts on the part of some Legal Entity.</skos:definition>
      <rdfs:subClassOf rdf:resource="http://www.omg.org/spec/EDMC-SR/FND/Parties/Parties/PartyInRole"/>
   </owl:Class>

   <owl:Class rdf:about="http://www.omg.org/spec/EDMC-SR/BE/LegalEntities/LegalPersons/StatutoryBody">
      <rdfs:label>Statutory Body</rdfs:label>
      <skos:definition>A legal person which is created and given legal personhood by act of statute.</skos:definition>
      <skos:editorialNote>The name exists and the meaning exists (verified) but we need to verify that this term does correspond to this concept. Otherwise there may not be a common name for these, since these are usually one off e.g. regulatory bodies created by some regulatory law. Editorial note: Body Corporates may be created by Act of Parliament - the instrument of incorporation in this case is the statute which creates the entity.</skos:editorialNote>
   </owl:Class>

   <owl:Class rdf:about="http://www.omg.org/spec/EDMC-SR/BE/LegalEntities/LegalPersons/NaturalPerson">
      <rdfs:label>Natural Person</rdfs:label>
      <rdfs:subClassOf rdf:resource="http://www.omg.org/spec/EDMC-SR/FND/AgentsAndPeople/People/Adult"/>
   </owl:Class>

   <!--Individuals-->

<owl:NamedIndividual rdf:about="http://www.omg.org/spec/EDMC-SR/BE/LegalEntities/LegalPersons/www.investorwords.com">
      <rdf:Type rdf:resource="http://www.edmcouncil.org/spec/EDMC-SR/FND/Publications/Publications/WebPage"/>
   </owl:NamedIndividual>

</rdf:RDF>