<?xml version="1.0" encoding="UTF-8"?>
<!DOCTYPE rdf:RDF [
	<!ENTITY fibo-bp-iss-trm "https://spec.edmcouncil.org/fibo/BP/SecuritiesIssuance/IssuanceProcessTerms/">
	<!ENTITY fibo-der-der-ex "https://spec.edmcouncil.org/fibo/DER/DerivativesContracts/ExerciseConventions/">
	<!ENTITY fibo-der-derx-dbx "https://spec.edmcouncil.org/fibo/DER/DerivativesContractsExt/DerivativesBasicsExt/">
	<!ENTITY fibo-der-rgt-raw "https://spec.edmcouncil.org/fibo/DER/RightsInstruments/RightsAndWarrants/">
	<!ENTITY fibo-fnd-accx-acc "https://spec.edmcouncil.org/fibo/FND/AccountingExt/AccountsMain/">
	<!ENTITY fibo-fnd-agr-ctr "https://spec.edmcouncil.org/fibo/FND/Agreements/Contracts/">
	<!ENTITY fibo-fnd-bus-pasx "https://spec.edmcouncil.org/fibo/FND/Business/ProductsAndServicesExt/">
	<!ENTITY fibo-fnd-math-math "https://spec.edmcouncil.org/fibo/FND/MathExt/Math/">
	<!ENTITY fibo-fnd-pty-pty "https://spec.edmcouncil.org/fibo/FND/Parties/Parties/">
	<!ENTITY fibo-fnd-ptyx-ptyx "https://spec.edmcouncil.org/fibo/FND/PartiesExt/PartyExtensions/">
	<!ENTITY fibo-fnd-rel-rel "https://spec.edmcouncil.org/fibo/FND/Relations/Relations/">
	<!ENTITY fibo-fnd-utl-av "https://spec.edmcouncil.org/fibo/FND/Utilities/AnnotationVocabulary/">
	<!ENTITY fibo-fnd-utlx-val "https://spec.edmcouncil.org/fibo/FND/UtilitiesExt/Values/">
	<!ENTITY fibo-sec-dbt-bo-bo "https://spec.edmcouncil.org/fibo/SEC/Debt/Bonds/BondsCommon/">
	<!ENTITY fibo-sec-dbt-dbt-iss "https://spec.edmcouncil.org/fibo/SEC/Debt/DebtFoundations/DebtIssuanceTerms/">
	<!ENTITY fibo-sec-eq-eq "https://spec.edmcouncil.org/fibo/SEC/Equities/EquityInstruments/">
	<!ENTITY fibo-sec-secx-assx "https://spec.edmcouncil.org/fibo/SEC/SecuritiesExt/SecurityAssetsExt/">
	<!ENTITY fibo-sec-secx-lisx "https://spec.edmcouncil.org/fibo/SEC/SecuritiesExt/SecuritiesListingsExt/">
	<!ENTITY fibo-sec-secx-sec "https://spec.edmcouncil.org/fibo/SEC/SecuritiesExt/SecuritiesExt/">
	<!ENTITY owl "http://www.w3.org/2002/07/owl#">
	<!ENTITY rdf "http://www.w3.org/1999/02/22-rdf-syntax-ns#">
	<!ENTITY rdfs "http://www.w3.org/2000/01/rdf-schema#">
	<!ENTITY skos "http://www.w3.org/2004/02/skos/core#">
	<!ENTITY xsd "http://www.w3.org/2001/XMLSchema#">
]>
<rdf:RDF xml:base="https://spec.edmcouncil.org/fibo/DER/RightsInstruments/RightsAndWarrants/"
	xmlns:fibo-bp-iss-trm="https://spec.edmcouncil.org/fibo/BP/SecuritiesIssuance/IssuanceProcessTerms/"
	xmlns:fibo-der-der-ex="https://spec.edmcouncil.org/fibo/DER/DerivativesContracts/ExerciseConventions/"
	xmlns:fibo-der-derx-dbx="https://spec.edmcouncil.org/fibo/DER/DerivativesContractsExt/DerivativesBasicsExt/"
	xmlns:fibo-der-rgt-raw="https://spec.edmcouncil.org/fibo/DER/RightsInstruments/RightsAndWarrants/"
	xmlns:fibo-fnd-accx-acc="https://spec.edmcouncil.org/fibo/FND/AccountingExt/AccountsMain/"
	xmlns:fibo-fnd-agr-ctr="https://spec.edmcouncil.org/fibo/FND/Agreements/Contracts/"
	xmlns:fibo-fnd-bus-pasx="https://spec.edmcouncil.org/fibo/FND/Business/ProductsAndServicesExt/"
	xmlns:fibo-fnd-math-math="https://spec.edmcouncil.org/fibo/FND/MathExt/Math/"
	xmlns:fibo-fnd-pty-pty="https://spec.edmcouncil.org/fibo/FND/Parties/Parties/"
	xmlns:fibo-fnd-ptyx-ptyx="https://spec.edmcouncil.org/fibo/FND/PartiesExt/PartyExtensions/"
	xmlns:fibo-fnd-rel-rel="https://spec.edmcouncil.org/fibo/FND/Relations/Relations/"
	xmlns:fibo-fnd-utl-av="https://spec.edmcouncil.org/fibo/FND/Utilities/AnnotationVocabulary/"
	xmlns:fibo-fnd-utlx-val="https://spec.edmcouncil.org/fibo/FND/UtilitiesExt/Values/"
	xmlns:fibo-sec-dbt-bo-bo="https://spec.edmcouncil.org/fibo/SEC/Debt/Bonds/BondsCommon/"
	xmlns:fibo-sec-dbt-dbt-iss="https://spec.edmcouncil.org/fibo/SEC/Debt/DebtFoundations/DebtIssuanceTerms/"
	xmlns:fibo-sec-eq-eq="https://spec.edmcouncil.org/fibo/SEC/Equities/EquityInstruments/"
	xmlns:fibo-sec-secx-assx="https://spec.edmcouncil.org/fibo/SEC/SecuritiesExt/SecurityAssetsExt/"
	xmlns:fibo-sec-secx-lisx="https://spec.edmcouncil.org/fibo/SEC/SecuritiesExt/SecuritiesListingsExt/"
	xmlns:fibo-sec-secx-sec="https://spec.edmcouncil.org/fibo/SEC/SecuritiesExt/SecuritiesExt/"
	xmlns:owl="http://www.w3.org/2002/07/owl#"
	xmlns:rdf="http://www.w3.org/1999/02/22-rdf-syntax-ns#"
	xmlns:rdfs="http://www.w3.org/2000/01/rdf-schema#"
	xmlns:skos="http://www.w3.org/2004/02/skos/core#"
	xmlns:xsd="http://www.w3.org/2001/XMLSchema#">
	
	<owl:Ontology rdf:about="https://spec.edmcouncil.org/fibo/DER/RightsInstruments/RightsAndWarrants/">
		<rdfs:label xml:lang="en">RightsAndWarrants</rdfs:label>
		<owl:imports rdf:resource="http://www.w3.org/2004/02/skos/core"/>
		<owl:imports rdf:resource="https://spec.edmcouncil.org/fibo/BP/SecuritiesIssuance/IssuanceProcessTerms/"/>
		<owl:imports rdf:resource="https://spec.edmcouncil.org/fibo/DER/DerivativesContracts/DerivativesBasics/"/>
		<owl:imports rdf:resource="https://spec.edmcouncil.org/fibo/DER/DerivativesContracts/ExerciseConventions/"/>
		<owl:imports rdf:resource="https://spec.edmcouncil.org/fibo/DER/DerivativesContractsExt/DerivativesBasicsExt/"/>
		<owl:imports rdf:resource="https://spec.edmcouncil.org/fibo/FBC/FinancialInstruments/FinancialInstruments/"/>
		<owl:imports rdf:resource="https://spec.edmcouncil.org/fibo/FND/AccountingExt/AccountsMain/"/>
		<owl:imports rdf:resource="https://spec.edmcouncil.org/fibo/FND/Agreements/Contracts/"/>
		<owl:imports rdf:resource="https://spec.edmcouncil.org/fibo/FND/MathExt/Math/"/>
		<owl:imports rdf:resource="https://spec.edmcouncil.org/fibo/FND/Parties/Parties/"/>
		<owl:imports rdf:resource="https://spec.edmcouncil.org/fibo/FND/PartiesExt/PartyExtensions/"/>
		<owl:imports rdf:resource="https://spec.edmcouncil.org/fibo/FND/Relations/Relations/"/>
		<owl:imports rdf:resource="https://spec.edmcouncil.org/fibo/FND/Utilities/AnnotationVocabulary/"/>
		<owl:imports rdf:resource="https://spec.edmcouncil.org/fibo/FND/UtilitiesExt/Values/"/>
		<owl:imports rdf:resource="https://spec.edmcouncil.org/fibo/SEC/Debt/Bonds/BondsCommon/"/>
		<owl:imports rdf:resource="https://spec.edmcouncil.org/fibo/SEC/Debt/DebtFoundations/DebtIssuanceTerms/"/>
		<owl:imports rdf:resource="https://spec.edmcouncil.org/fibo/SEC/Equities/EquityInstruments/"/>
		<owl:imports rdf:resource="https://spec.edmcouncil.org/fibo/SEC/Securities/SecuritiesListings/"/>
		<owl:imports rdf:resource="https://spec.edmcouncil.org/fibo/SEC/Securities/SecurityAssets/"/>
		<owl:imports rdf:resource="https://spec.edmcouncil.org/fibo/SEC/SecuritiesExt/SecuritiesExt/"/>
		<owl:imports rdf:resource="https://spec.edmcouncil.org/fibo/SEC/SecuritiesExt/SecuritiesListingsExt/"/>
		<owl:imports rdf:resource="https://spec.edmcouncil.org/fibo/SEC/SecuritiesExt/SecurityAssetsExt/"/>
		<owl:versionIRI rdf:resource="https://spec.edmcouncil.org/fibo/DER/RightsInstruments/RightsAndWarrants/"/>
		<fibo-fnd-utl-av:hasMaturityLevel rdf:resource="&fibo-fnd-utl-av;Informative"/>
	</owl:Ontology>
	
	<owl:Class rdf:about="&fibo-der-rgt-raw;AllotmentRight">
		<rdfs:subClassOf rdf:resource="&fibo-der-rgt-raw;StockholdersRightsInstrument"/>
		<rdfs:subClassOf>
			<owl:Restriction>
				<owl:onProperty rdf:resource="&fibo-der-rgt-raw;numberOfSecuritiesDeterminedBy"/>
				<owl:someValuesFrom rdf:resource="&fibo-der-rgt-raw;AllotmentRightFormula"/>
			</owl:Restriction>
		</rdfs:subClassOf>
		<rdfs:label xml:lang="en">allotment right</rdfs:label>
		<skos:definition xml:lang="en">Privileges allotted to existing security holders, entitling them to receive new securities free of charge.</skos:definition>
	</owl:Class>
	
	<owl:Class rdf:about="&fibo-der-rgt-raw;AllotmentRightFormula">
		<rdfs:subClassOf rdf:resource="&fibo-fnd-math-math;Formula"/>
		<rdfs:label xml:lang="en">allotment right formula</rdfs:label>
		<skos:definition xml:lang="en">A formula used to calculate the number of securities for an Allotment Right, based on the number of these instruments that the holder holds. Conesnsus:Review</skos:definition>
	</owl:Class>
	
	<owl:Class rdf:about="&fibo-der-rgt-raw;AllotmentRightHolder">
		<rdfs:subClassOf rdf:resource="&fibo-der-rgt-raw;StockholdersRightsInstrumentHolder"/>
		<rdfs:subClassOf>
			<owl:Restriction>
				<owl:onProperty rdf:resource="&fibo-der-rgt-raw;isByVirtueOfBeing"/>
				<owl:someValuesFrom rdf:resource="https://spec.edmcouncil.org/fibo/SEC/Securities/SecurityAssets/SecurityHolder"/>
			</owl:Restriction>
		</rdfs:subClassOf>
		<rdfs:label xml:lang="en">allotment right holder</rdfs:label>
		<skos:definition xml:lang="en">The party which is the holder of an allotment right. This is identified as being a party which is also an existing holder of the security identified as the underlying security.</skos:definition>
	</owl:Class>
	
	<owl:Class rdf:about="&fibo-der-rgt-raw;CommodityWarrant">
		<rdfs:subClassOf rdf:resource="&fibo-der-rgt-raw;Warrant"/>
		<rdfs:subClassOf>
			<owl:Restriction>
				<owl:onProperty rdf:resource="&fibo-der-rgt-raw;hasExerciseTerms"/>
				<owl:someValuesFrom rdf:resource="&fibo-der-rgt-raw;CommodityWarrantExerciseTerms"/>
			</owl:Restriction>
		</rdfs:subClassOf>
		<rdfs:label xml:lang="en">commodity warrant</rdfs:label>
		<skos:definition xml:lang="en">A derivative based on commodities contracts traded on exchanges.</skos:definition>
		<fibo-fnd-utl-av:explanatoryNote xml:lang="en">Example: Commodity Warrants Australia (CWA) is a locally owned outfit that has been in business for 18 months. It sells warrants based on 12 commodities and financial markets - crude oil, gold, silver, live cattle, corn, orange juice, soy, coffee, cocoa, the Dow Jones Industrial Average, the NASDAQ Composite Index and the S&amp;P 500 Index</fibo-fnd-utl-av:explanatoryNote>
	</owl:Class>
	
	<owl:Class rdf:about="&fibo-der-rgt-raw;CommodityWarrantExerciseTerms">
		<rdfs:subClassOf rdf:resource="&fibo-der-rgt-raw;WarrantExerciseTermsSet"/>
		<rdfs:subClassOf>
			<owl:Restriction>
				<owl:onProperty rdf:resource="&fibo-der-rgt-raw;delivery"/>
				<owl:someValuesFrom rdf:resource="&fibo-fnd-accx-acc;CashCurrency"/>
			</owl:Restriction>
		</rdfs:subClassOf>
		<rdfs:label xml:lang="en">commodity warrant exercise terms</rdfs:label>
		<skos:definition xml:lang="en">Terms setting out how a commodity warrant may be exercised, including the form which delivery takes.</skos:definition>
	</owl:Class>
	
	<owl:Class rdf:about="&fibo-der-rgt-raw;CompanyWarrant">
		<rdfs:subClassOf rdf:resource="&fibo-der-rgt-raw;Warrant"/>
		<rdfs:subClassOf>
			<owl:Restriction>
				<owl:onProperty rdf:resource="&fibo-der-rgt-raw;hasExerciseTerms"/>
				<owl:someValuesFrom rdf:resource="&fibo-der-rgt-raw;CompanyWarrantExerciseTermsSet"/>
			</owl:Restriction>
		</rdfs:subClassOf>
		<rdfs:subClassOf>
			<owl:Restriction>
				<owl:onProperty rdf:resource="&fibo-der-rgt-raw;hasWarrantUnderlying"/>
				<owl:someValuesFrom rdf:resource="https://spec.edmcouncil.org/fibo/FBC/FinancialInstruments/FinancialInstruments/Security"/>
			</owl:Restriction>
		</rdfs:subClassOf>
		<rdfs:label xml:lang="en">company warrant</rdfs:label>
		<owl:disjointWith rdf:resource="&fibo-der-rgt-raw;CoveredWarrant"/>
		<skos:definition xml:lang="en">Warrants which are issued by the issuer of the underlying.</skos:definition>
	</owl:Class>
	
	<owl:Class rdf:about="&fibo-der-rgt-raw;CompanyWarrantExerciseTermsSet">
		<rdfs:subClassOf rdf:resource="&fibo-der-rgt-raw;WarrantExerciseTermsSet"/>
		<rdfs:subClassOf>
			<owl:Restriction>
				<owl:onProperty rdf:resource="&fibo-der-rgt-raw;delivery"/>
				<owl:someValuesFrom rdf:resource="https://spec.edmcouncil.org/fibo/FBC/FinancialInstruments/FinancialInstruments/Security"/>
			</owl:Restriction>
		</rdfs:subClassOf>
		<rdfs:label xml:lang="en">company warrant exercise terms set</rdfs:label>
		<owl:disjointWith rdf:resource="&fibo-der-rgt-raw;CoveredWarrantExerciseTerms"/>
		<skos:definition xml:lang="en">Terms setting out how a company warrant or naked warrant may be exercised, including the form which delivery takes.</skos:definition>
	</owl:Class>
	
	<owl:Class rdf:about="&fibo-der-rgt-raw;CoveredWarrant">
		<rdfs:subClassOf rdf:resource="&fibo-der-rgt-raw;Warrant"/>
		<rdfs:subClassOf>
			<owl:Restriction>
				<owl:onProperty rdf:resource="&fibo-der-rgt-raw;hasExerciseTerms"/>
				<owl:someValuesFrom rdf:resource="&fibo-der-rgt-raw;CoveredWarrantExerciseTerms"/>
			</owl:Restriction>
		</rdfs:subClassOf>
		<rdfs:subClassOf>
			<owl:Restriction>
				<owl:onProperty rdf:resource="&fibo-der-rgt-raw;hasWarrantUnderlying"/>
				<owl:someValuesFrom rdf:resource="https://spec.edmcouncil.org/fibo/FBC/FinancialInstruments/FinancialInstruments/Security"/>
			</owl:Restriction>
		</rdfs:subClassOf>
		<rdfs:label xml:lang="en">covered warrant</rdfs:label>
	</owl:Class>
	
	<owl:Class rdf:about="&fibo-der-rgt-raw;CoveredWarrantExerciseTerms">
		<rdfs:subClassOf rdf:resource="&fibo-der-rgt-raw;WarrantExerciseTermsSet"/>
		<rdfs:subClassOf>
			<owl:Restriction>
				<owl:onProperty rdf:resource="&fibo-der-rgt-raw;delivery"/>
				<owl:someValuesFrom rdf:resource="https://spec.edmcouncil.org/fibo/FBC/FinancialInstruments/FinancialInstruments/Security"/>
			</owl:Restriction>
		</rdfs:subClassOf>
		<rdfs:label xml:lang="en">covered warrant exercise terms</rdfs:label>
	</owl:Class>
	
	<owl:Class rdf:about="&fibo-der-rgt-raw;EntitlementRightsInstrument">
		<rdfs:subClassOf rdf:resource="https://spec.edmcouncil.org/fibo/FBC/FinancialInstruments/FinancialInstruments/DerivativeInstrument"/>
		<rdfs:subClassOf rdf:resource="https://spec.edmcouncil.org/fibo/FBC/FinancialInstruments/FinancialInstruments/Security"/>
		<rdfs:label xml:lang="en">entitlement rights instrument</rdfs:label>
		<skos:definition xml:lang="en">A security giving the holder of that security the entitlement to purchase or sell back to the issuer new securities or some other commodity or instrument at a predetermined price.</skos:definition>
	</owl:Class>
	
	<owl:Class rdf:about="&fibo-der-rgt-raw;ExchangeTradedWarrant">
		<rdfs:subClassOf rdf:resource="&fibo-der-rgt-raw;Warrant"/>
		<rdfs:subClassOf rdf:resource="https://spec.edmcouncil.org/fibo/SEC/Securities/SecuritiesListings/ExchangeTradedSecurity"/>
		<rdfs:subClassOf>
			<owl:Restriction>
				<owl:onProperty rdf:resource="&fibo-der-rgt-raw;hasListing"/>
				<owl:someValuesFrom rdf:resource="&fibo-der-rgt-raw;WarrantListing"/>
			</owl:Restriction>
		</rdfs:subClassOf>
		<rdfs:label xml:lang="en">exchange traded warrant</rdfs:label>
		<skos:definition xml:lang="en">A warrant which is traded on a securities exchange.</skos:definition>
		<fibo-fnd-utl-av:explanatoryNote xml:lang="en">This may be any kind of warrant except a (usually) Company Warrant. According to notes on Traditional Wwarrant: Warrants may be privately issued and may not necessarily be traded on an exchange. (Wikipedia)</fibo-fnd-utl-av:explanatoryNote>
	</owl:Class>
	
	<owl:Class rdf:about="&fibo-der-rgt-raw;PurchaseRight">
		<rdfs:subClassOf rdf:resource="&fibo-der-rgt-raw;StockholdersRightsInstrument"/>
		<rdfs:label xml:lang="en">purchase right</rdfs:label>
		<skos:definition xml:lang="en">Anti-takeover device that gives a prospective acquireeâ€™s shareholders the right to buy usually shares of the firm or shares of anyone who acquires the firm at a deep discount to their fair market value.</skos:definition>
		<fibo-fnd-utl-av:explanatoryNote xml:lang="en">The underlying is usually shares but this not necessarily the case. Also known as &quot;Poison Pill&quot;.</fibo-fnd-utl-av:explanatoryNote>
	</owl:Class>
	
	<owl:Class rdf:about="&fibo-der-rgt-raw;StockholdersRightsInstrument">
		<rdfs:subClassOf rdf:resource="&fibo-der-rgt-raw;EntitlementRightsInstrument"/>
		<rdfs:subClassOf>
			<owl:Restriction>
				<owl:onProperty rdf:resource="&fibo-bp-iss-trm;issuer"/>
				<owl:someValuesFrom rdf:resource="&fibo-der-rgt-raw;StockholdersRightsInstrumentIssuer"/>
			</owl:Restriction>
		</rdfs:subClassOf>
		<rdfs:subClassOf>
			<owl:Restriction>
				<owl:onProperty rdf:resource="&fibo-der-rgt-raw;givesTheRightToBuy"/>
				<owl:someValuesFrom rdf:resource="https://spec.edmcouncil.org/fibo/FBC/FinancialInstruments/FinancialInstruments/Security"/>
			</owl:Restriction>
		</rdfs:subClassOf>
		<rdfs:subClassOf>
			<owl:Restriction>
				<owl:onProperty rdf:resource="&fibo-sec-secx-assx;hasHolder"/>
				<owl:someValuesFrom rdf:resource="&fibo-der-rgt-raw;StockholdersRightsInstrumentHolder"/>
			</owl:Restriction>
		</rdfs:subClassOf>
		<rdfs:label xml:lang="en">stockholders rights instrument</rdfs:label>
		<skos:definition xml:lang="en">A security giving stockholders entitlement to purchase new securities issued by the corporation at a predetermined price (normally less than the current market price) in proportion to the number of securities already owned.</skos:definition>
		<fibo-fnd-utl-av:explanatoryNote xml:lang="en">Stockholders may sell these to non stockholders if they wish. Rights are issued only for a short period of time, after which they expire.</fibo-fnd-utl-av:explanatoryNote>
	</owl:Class>
	
	<owl:Class rdf:about="&fibo-der-rgt-raw;StockholdersRightsInstrumentHolder">
		<rdfs:subClassOf rdf:resource="https://spec.edmcouncil.org/fibo/SEC/Securities/SecurityAssets/SecurityHolder"/>
		<rdfs:label xml:lang="en">stockholders rights instrument holder</rdfs:label>
		<skos:definition xml:lang="en">A party which is the holder of a Stockholders Rights instrument.</skos:definition>
	</owl:Class>
	
	<owl:Class rdf:about="&fibo-der-rgt-raw;StockholdersRightsInstrumentIssuer">
		<rdfs:subClassOf rdf:resource="&fibo-bp-iss-trm;SecurityIssuer"/>
		<rdfs:label xml:lang="en">stockholders rights instrument issuer</rdfs:label>
		<skos:definition xml:lang="en">The party which is the issuer of a Stockholders Rights instrument.</skos:definition>
		<skos:editorialNote xml:lang="en">Specializes the term &quot;Issuer&quot; for different instrument classes; this specialization is not present in ISO FIBIM where the term is &quot;Issuer&quot; in each case.</skos:editorialNote>
	</owl:Class>
	
	<owl:Class rdf:about="&fibo-der-rgt-raw;SubscriptionRight">
		<rdfs:subClassOf rdf:resource="&fibo-der-rgt-raw;StockholdersRightsInstrument"/>
		<rdfs:subClassOf>
			<owl:Restriction>
				<owl:onProperty rdf:resource="&fibo-der-rgt-raw;givesRightToBuy"/>
				<owl:someValuesFrom rdf:resource="&fibo-sec-eq-eq;Share"/>
			</owl:Restriction>
		</rdfs:subClassOf>
		<rdfs:label xml:lang="en">subscription right</rdfs:label>
		<skos:definition xml:lang="en">Privileges allotted to existing security holders, entitling them to subscribe to new securities at a price normally lower than the prevailing market price.</skos:definition>
		<skos:editorialNote xml:lang="en">Why prevailing? It could be a new security of exactly the same class. Is this always new securities? Notes May 25: May be more an accounting or legal term for bonus issue, more accurate than scrip or bonus issue which reflects what happens in the books of the company. THis would mean that capitalization issue is seemingly synonymous with Bonus Issue / Scrip Issue (see moneytterms.co.uk which says that capitalization is less common but more correct, for scrip. &quot;The share capital on the balance sheet has to increate by the nominal value of the newly issued shares. This is balanced by an equal decrease in another part of hte shareholder&apos;s funds such as retained income of valuation reserves&quot;</skos:editorialNote>
	</owl:Class>
	
	<owl:Class rdf:about="&fibo-der-rgt-raw;SubscriptionRightHolder">
		<rdfs:subClassOf rdf:resource="&fibo-der-rgt-raw;StockholdersRightsInstrumentHolder"/>
		<rdfs:subClassOf>
			<owl:Restriction>
				<owl:onProperty rdf:resource="&fibo-der-rgt-raw;isByVirtueOfBeing"/>
				<owl:someValuesFrom rdf:resource="https://spec.edmcouncil.org/fibo/SEC/Securities/SecurityAssets/SecurityHolder"/>
			</owl:Restriction>
		</rdfs:subClassOf>
		<rdfs:label xml:lang="en">subscription right holder</rdfs:label>
		<skos:definition xml:lang="en">The party which is the holder of a subscription right. This is identified as being a party which is also an existing holder of the security identified as the underlying security.</skos:definition>
	</owl:Class>
	
	<owl:Class rdf:about="&fibo-der-rgt-raw;ThirdPartyWarrantIssuer">
		<rdfs:subClassOf rdf:resource="&fibo-der-rgt-raw;WarrantIssuer"/>
		<rdfs:label xml:lang="en">third party warrant issuer</rdfs:label>
		<owl:disjointWith rdf:resource="&fibo-der-rgt-raw;UnderlyingIssuer"/>
	</owl:Class>
	
	<owl:Class rdf:about="&fibo-der-rgt-raw;TraditionalWarrant">
		<rdfs:subClassOf rdf:resource="&fibo-der-rgt-raw;CompanyWarrant"/>
		<rdfs:label xml:lang="en">traditional warrant</rdfs:label>
		<skos:definition xml:lang="en">Financial instruments which permit the holder to purchase or sell back to the issuer a specified amount of a share.</skos:definition>
		<fibo-fnd-utl-av:explanatoryNote xml:lang="en">Warrants may be privately issued and may not necessarily be traded on an exchange. From Wikipedia: A warrant issued with a bond gives the holder the right to purchase equity shares issued by the company that issued the bond with the warrant.</fibo-fnd-utl-av:explanatoryNote>
	</owl:Class>
	
	<owl:Class rdf:about="&fibo-der-rgt-raw;UnderlyingIssuer">
		<rdfs:subClassOf rdf:resource="&fibo-der-rgt-raw;WarrantIssuer"/>
		<rdfs:subClassOf>
			<owl:Restriction>
				<owl:onProperty rdf:resource="&fibo-der-rgt-raw;identifiedAs"/>
				<owl:someValuesFrom rdf:resource="&fibo-bp-iss-trm;SecurityIssuer"/>
			</owl:Restriction>
		</rdfs:subClassOf>
		<rdfs:label xml:lang="en">underlying issuer</rdfs:label>
		<skos:definition xml:lang="en">A party which is the issuer of a Covered Warrant. This party is by definition the issuer of the underlying securities.</skos:definition>
		<skos:editorialNote xml:lang="en">Specializes the term &quot;Issuer&quot; for different instrument classes; this specialization is not present in ISO FIBIM where the term is &quot;Issuer&quot; in each case.</skos:editorialNote>
	</owl:Class>
	
	<owl:Class rdf:about="&fibo-der-rgt-raw;Warrant">
		<rdfs:subClassOf rdf:resource="&fibo-der-rgt-raw;EntitlementRightsInstrument"/>
		<rdfs:subClassOf>
			<owl:Restriction>
				<owl:onProperty rdf:resource="&fibo-bp-iss-trm;issuer"/>
				<owl:someValuesFrom rdf:resource="&fibo-der-rgt-raw;WarrantIssuer"/>
			</owl:Restriction>
		</rdfs:subClassOf>
		<rdfs:subClassOf>
			<owl:Restriction>
				<owl:onProperty rdf:resource="&fibo-der-rgt-raw;hasExerciseTerms"/>
				<owl:someValuesFrom rdf:resource="&fibo-der-rgt-raw;WarrantExerciseTermsSet"/>
			</owl:Restriction>
		</rdfs:subClassOf>
		<rdfs:subClassOf>
			<owl:Restriction>
				<owl:onProperty rdf:resource="&fibo-der-rgt-raw;hasWarrantUnderlying"/>
				<owl:someValuesFrom rdf:resource="https://spec.edmcouncil.org/fibo/DER/DerivativesContracts/DerivativesBasics/Underlier"/>
			</owl:Restriction>
		</rdfs:subClassOf>
		<rdfs:label xml:lang="en">warrant</rdfs:label>
		<skos:definition xml:lang="en">Financial instruments which permit the holder to purchase or sell back to the issuer a specified amount of a financial instrument, commodity, currency or other during a specified period at a specified price.</skos:definition>
		<fibo-fnd-utl-av:explanatoryNote xml:lang="en">Warrants are for any kind of instrument. Warrants may be privately issued and may not necessarily be traded on an exchange.</fibo-fnd-utl-av:explanatoryNote>
	</owl:Class>
	
	<owl:Class rdf:about="&fibo-der-rgt-raw;WarrantExerciseTermsSet">
		<rdfs:subClassOf rdf:resource="&fibo-fnd-agr-ctr;ContractualCommitment"/>
		<rdfs:subClassOf>
			<owl:Restriction>
				<owl:onProperty rdf:resource="&fibo-der-rgt-raw;delivery"/>
				<owl:someValuesFrom rdf:resource="https://spec.edmcouncil.org/fibo/FBC/FinancialInstruments/FinancialInstruments/FinancialInstrument"/>
			</owl:Restriction>
		</rdfs:subClassOf>
		<rdfs:subClassOf>
			<owl:Restriction>
				<owl:onProperty rdf:resource="&fibo-der-rgt-raw;hasExerciseConvention"/>
				<owl:someValuesFrom rdf:resource="&fibo-der-der-ex;ExerciseDatesConvention"/>
			</owl:Restriction>
		</rdfs:subClassOf>
		<rdfs:label xml:lang="en">warrant exercise terms set</rdfs:label>
		<skos:definition xml:lang="en">Terms setting out how a warrant instrument may be exercised. Further Notes Exercise terms as defined here also cover the automatic exercise of the warrant in the event of its expiry. These terms include the exercise style (FIBIM = OptionStyle type OptionStyleCode) and the delivery.</skos:definition>
	</owl:Class>
	
	<owl:Class rdf:about="&fibo-der-rgt-raw;WarrantIssuer">
		<rdfs:subClassOf rdf:resource="&fibo-bp-iss-trm;SecurityIssuer"/>
		<rdfs:label xml:lang="en">warrant issuer</rdfs:label>
		<skos:definition xml:lang="en">The issuer of a Warrant. This is defined in terms of what individual entity is the issuer and also what other roles they may or may not play for a specific type of warranty, specifically whether or not they are also the issuer of the underlying, if the underlying is a security.</skos:definition>
		<skos:editorialNote xml:lang="en">Specializes the term &quot;Issuer&quot; for different instrument classes; this specialization is not present in ISO FIBIM where the term is &quot;Issuer&quot; in each case.</skos:editorialNote>
	</owl:Class>
	
	<owl:Class rdf:about="&fibo-der-rgt-raw;WarrantListing">
		<rdfs:subClassOf rdf:resource="https://spec.edmcouncil.org/fibo/SEC/Securities/SecuritiesListings/SecurityListing"/>
		<rdfs:label xml:lang="en">warrant listing</rdfs:label>
		<skos:definition xml:lang="en">The listing of a warrant on a securities exchange. Action: confirm whether all the facts shown for listing of tradable securities generally, apply to the listing of a warrant. Also determine whether any of the terms in Listing need to be specialized or added to for Warrant Listing.</skos:definition>
	</owl:Class>
	
	<owl:ObjectProperty rdf:about="&fibo-der-rgt-raw;delivery">
		<rdfs:label xml:lang="en">delivery</rdfs:label>
		<rdfs:domain rdf:resource="&fibo-der-rgt-raw;WarrantExerciseTermsSet"/>
		<rdfs:range rdf:resource="https://spec.edmcouncil.org/fibo/FBC/FinancialInstruments/FinancialInstruments/FinancialInstrument"/>
	</owl:ObjectProperty>
	
	<owl:DatatypeProperty rdf:about="&fibo-der-rgt-raw;expiryDate">
		<rdfs:label xml:lang="en">expiry date</rdfs:label>
		<rdfs:domain rdf:resource="&fibo-der-rgt-raw;EntitlementRightsInstrument"/>
		<skos:definition xml:lang="en">Legal expiry of the Contract.</skos:definition>
	</owl:DatatypeProperty>
	
	<owl:DatatypeProperty rdf:about="&fibo-der-rgt-raw;expiryDate.1">
		<rdfs:label xml:lang="en">expiry date</rdfs:label>
		<rdfs:domain rdf:resource="&fibo-der-rgt-raw;Warrant"/>
		<skos:definition xml:lang="en">Expiry date of the warrant. This is the last date on which the holder may exercise the right to buy or sell back the underlying security.</skos:definition>
	</owl:DatatypeProperty>
	
	<owl:ObjectProperty rdf:about="&fibo-der-rgt-raw;formulaText">
		<rdfs:label xml:lang="en">formula text</rdfs:label>
		<rdfs:domain rdf:resource="&fibo-der-rgt-raw;AllotmentRightFormula"/>
		<rdfs:range rdf:resource="&fibo-fnd-utlx-val;TextValue"/>
		<skos:definition xml:lang="en">The formula stated as text.</skos:definition>
	</owl:ObjectProperty>
	
	<owl:ObjectProperty rdf:about="&fibo-der-rgt-raw;givesRightToBuy">
		<rdfs:subPropertyOf rdf:resource="&fibo-der-rgt-raw;givesTheRightToBuy"/>
		<rdfs:label xml:lang="en">gives right to buy</rdfs:label>
		<rdfs:domain rdf:resource="&fibo-der-rgt-raw;SubscriptionRight"/>
		<rdfs:range rdf:resource="&fibo-sec-eq-eq;Share"/>
	</owl:ObjectProperty>
	
	<owl:ObjectProperty rdf:about="&fibo-der-rgt-raw;givesTheRightToBuy">
		<rdfs:subPropertyOf rdf:resource="https://spec.edmcouncil.org/fibo/DER/DerivativesContracts/DerivativesBasics/hasUnderlier"/>
		<rdfs:label xml:lang="en">gives the right to buy</rdfs:label>
		<rdfs:domain rdf:resource="&fibo-der-rgt-raw;StockholdersRightsInstrument"/>
		<rdfs:range rdf:resource="https://spec.edmcouncil.org/fibo/FBC/FinancialInstruments/FinancialInstruments/Security"/>
	</owl:ObjectProperty>
	
	<owl:ObjectProperty rdf:about="&fibo-der-rgt-raw;hasExerciseConvention">
		<rdfs:subPropertyOf rdf:resource="&fibo-fnd-agr-ctr;isQualifiedBy"/>
		<rdfs:label xml:lang="en">has exercise convention</rdfs:label>
		<rdfs:domain rdf:resource="&fibo-der-rgt-raw;WarrantExerciseTermsSet"/>
		<rdfs:range rdf:resource="&fibo-der-der-ex;ExerciseDatesConvention"/>
	</owl:ObjectProperty>
	
	<owl:ObjectProperty rdf:about="&fibo-der-rgt-raw;hasExerciseTerms">
		<rdfs:subPropertyOf rdf:resource="&fibo-fnd-agr-ctr;hasContractualElement"/>
		<rdfs:label xml:lang="en">has exercise terms</rdfs:label>
		<rdfs:domain rdf:resource="&fibo-der-rgt-raw;Warrant"/>
		<rdfs:range rdf:resource="&fibo-der-rgt-raw;WarrantExerciseTermsSet"/>
	</owl:ObjectProperty>
	
	<owl:ObjectProperty rdf:about="&fibo-der-rgt-raw;hasListing">
		<rdfs:label xml:lang="en">has listing</rdfs:label>
		<rdfs:domain rdf:resource="&fibo-der-rgt-raw;ExchangeTradedWarrant"/>
		<rdfs:range rdf:resource="&fibo-der-rgt-raw;WarrantListing"/>
	</owl:ObjectProperty>
	
	<owl:ObjectProperty rdf:about="&fibo-der-rgt-raw;hasWarrantUnderlying">
		<rdfs:subPropertyOf rdf:resource="https://spec.edmcouncil.org/fibo/DER/DerivativesContracts/DerivativesBasics/hasUnderlier"/>
		<rdfs:label xml:lang="en">has warrant underlying</rdfs:label>
		<rdfs:domain rdf:resource="&fibo-der-rgt-raw;Warrant"/>
		<rdfs:range rdf:resource="https://spec.edmcouncil.org/fibo/DER/DerivativesContracts/DerivativesBasics/Underlier"/>
	</owl:ObjectProperty>
	
	<owl:ObjectProperty rdf:about="&fibo-der-rgt-raw;identifiedAs">
		<rdfs:label xml:lang="en">identified as</rdfs:label>
		<rdfs:domain rdf:resource="&fibo-der-rgt-raw;UnderlyingIssuer"/>
		<rdfs:range rdf:resource="&fibo-bp-iss-trm;SecurityIssuer"/>
	</owl:ObjectProperty>
	
	<owl:ObjectProperty rdf:about="&fibo-der-rgt-raw;isByVirtueOfBeing">
		<rdfs:subPropertyOf rdf:resource="&fibo-fnd-ptyx-ptyx;hasRelatedParty"/>
		<rdfs:label xml:lang="en">is by virtue of being</rdfs:label>
		<rdfs:domain rdf:resource="&fibo-der-rgt-raw;StockholdersRightsInstrumentHolder"/>
		<rdfs:range rdf:resource="https://spec.edmcouncil.org/fibo/SEC/Securities/SecurityAssets/SecurityHolder"/>
	</owl:ObjectProperty>
	
	<owl:ObjectProperty rdf:about="&fibo-der-rgt-raw;numberOfSecurities">
		<rdfs:label xml:lang="en">number of securities</rdfs:label>
		<rdfs:domain rdf:resource="&fibo-der-rgt-raw;AllotmentRight"/>
		<rdfs:range rdf:resource="&fibo-fnd-utlx-val;DecimalValue"/>
		<skos:definition xml:lang="en">The number of securities based on the number of these instruments that the holder holds.</skos:definition>
	</owl:ObjectProperty>
	
	<owl:ObjectProperty rdf:about="&fibo-der-rgt-raw;numberOfSecuritiesDeterminedBy">
		<rdfs:subPropertyOf rdf:resource="&fibo-fnd-agr-ctr;hasContractualElement"/>
		<rdfs:label xml:lang="en">number of securities determined by</rdfs:label>
		<rdfs:domain rdf:resource="&fibo-der-rgt-raw;AllotmentRight"/>
		<rdfs:range rdf:resource="&fibo-der-rgt-raw;AllotmentRightFormula"/>
	</owl:ObjectProperty>
	
	<owl:ObjectProperty rdf:about="&fibo-der-rgt-raw;oversubscribeOption">
		<rdfs:label xml:lang="en">oversubscribe option</rdfs:label>
		<rdfs:domain rdf:resource="&fibo-der-rgt-raw;StockholdersRightsInstrument"/>
		<rdfs:range rdf:resource="&fibo-fnd-utlx-val;TrueFalseValue"/>
		<skos:definition xml:lang="en">Option whereby the holders of the rights instrument may get securities in the event that other right holders choose not to subscribe to theirs.</skos:definition>
	</owl:ObjectProperty>
	
	<owl:ObjectProperty rdf:about="&fibo-der-rgt-raw;perpetualMaturity">
		<rdfs:label xml:lang="en">perpetual maturity</rdfs:label>
		<rdfs:domain rdf:resource="&fibo-der-rgt-raw;Warrant"/>
		<rdfs:range rdf:resource="&fibo-fnd-utlx-val;TrueFalseValue"/>
		<skos:definition xml:lang="en">Whether this is a perpetual warrant, in other words it has no expiry date.</skos:definition>
	</owl:ObjectProperty>
	
	<owl:ObjectProperty rdf:about="&fibo-der-rgt-raw;purchasePrice">
		<rdfs:label xml:lang="en">purchase price</rdfs:label>
		<rdfs:domain rdf:resource="&fibo-der-rgt-raw;PurchaseRight"/>
		<rdfs:range rdf:resource="&fibo-fnd-accx-acc;Price"/>
		<skos:definition xml:lang="en">The price at which the holder of the Purchase Right may purchase the underlying security.</skos:definition>
	</owl:ObjectProperty>
	
	<owl:ObjectProperty rdf:about="&fibo-der-rgt-raw;purchasePrice.1">
		<rdfs:label xml:lang="en">purchase price</rdfs:label>
		<rdfs:domain rdf:resource="&fibo-der-rgt-raw;SubscriptionRight"/>
		<rdfs:range rdf:resource="&fibo-fnd-accx-acc;Price"/>
		<skos:definition xml:lang="en">The price at which the holder of the Subscription Right may purchase the underlying security.</skos:definition>
	</owl:ObjectProperty>
	
	<owl:ObjectProperty rdf:about="&fibo-der-rgt-raw;putWarrant">
		<rdfs:label xml:lang="en">put warrant</rdfs:label>
		<rdfs:domain rdf:resource="&fibo-der-rgt-raw;Warrant"/>
		<rdfs:range rdf:resource="&fibo-fnd-utlx-val;TrueFalseValue"/>
		<skos:definition xml:lang="en">If Yes, this warrant gives the holder the right to sell the underlying security back to the issuer at a predetermined price; if No, the warrant gives the holder the right to purchase the instrument at the predetermined price (a call warrant).</skos:definition>
	</owl:ObjectProperty>
	
	<owl:ObjectProperty rdf:about="&fibo-der-rgt-raw;ratio">
		<rdfs:label xml:lang="en">ratio</rdfs:label>
		<rdfs:domain rdf:resource="&fibo-der-rgt-raw;CompanyWarrant"/>
		<rdfs:domain rdf:resource="&fibo-der-rgt-raw;CoveredWarrant"/>
		<rdfs:range rdf:resource="&fibo-fnd-utlx-val;DecimalValue"/>
		<skos:definition xml:lang="en">The ratio of warrant units to underlying security units for delivery when the warrant is exercised.</skos:definition>
	</owl:ObjectProperty>

</rdf:RDF>