<?xml version="1.0" encoding="UTF-8"?>
  
<!DOCTYPE rdf:RDF [
    <!ENTITY fibo-be-corp-corp "http://spec.edmcouncil.org/fibo/red/be/corporations/corporations/">
    <!ENTITY fibo-fnd-info-sch "http://spec.edmcouncil.org/fibo/red/fnd/information/schemes/">
    <!ENTITY fibo-be-le-fbo "http://spec.edmcouncil.org/fibo/red/be/legal-entities/formal-business-organizations/">
    <!ENTITY fibo-be-le-cb "http://spec.edmcouncil.org/fibo/red/be/legal-entities/corporate-bodies/">
    <!ENTITY fibo-fnd-rel-rel "http://spec.edmcouncil.org/fibo/red/fnd/relations/relations/">
    <!ENTITY fibo-fnd-law-jur "http://spec.edmcouncil.org/fibo/red/fnd/law/jurisdictions/">
    <!ENTITY fibo-fnd-acc-cur "http://spec.edmcouncil.org/fibo/red/fnd/accounting/currency-amount/">
    <!ENTITY fibo-fnd-utl-bt "http://spec.edmcouncil.org/fibo/red/fnd/utilities/business-facing-types/">
]>

<rdf:RDF xmlns:xsd="http://www.w3.org/2001/XMLSchema#"
         xmlns:sm="http://www.omg.org/techprocess/ab/SpecificationMetadata/"
         xmlns:xs="http://www.w3.org/2001/XMLSchema"
         xmlns:fibo-fnd-utl-av="http://www.omg.org/spec/EDMC-FIBO/FND/Utilities/AnnotationVocabulary/"
         xmlns:rdf="http://www.w3.org/1999/02/22-rdf-syntax-ns#"
         xmlns:rdfs="http://www.w3.org/2000/01/rdf-schema#"
         xmlns:owl="http://www.w3.org/2002/07/owl#"
         xmlns:skos="http://www.w3.org/2004/02/skos/core#"
         xmlns:dc="http://purl.org/dc/terms/"
         xml:base="http://spec.edmcouncil.org/fibo/red/be/corporations/corporations/">

   <owl:Ontology rdf:about="http://spec.edmcouncil.org/fibo/red/be/corporations/corporations/">
      <owl:imports rdf:resource="http://spec.edmcouncil.org/fibo/red/fnd/information/schemes/"/>
      <owl:imports rdf:resource="http://spec.edmcouncil.org/fibo/red/be/legal-entities/formal-business-organizations/"/>
      <owl:imports rdf:resource="http://spec.edmcouncil.org/fibo/red/be/legal-entities/corporate-bodies/"/>
      <owl:imports rdf:resource="http://spec.edmcouncil.org/fibo/red/fnd/relations/relations/"/>
      <owl:imports rdf:resource="http://spec.edmcouncil.org/fibo/red/fnd/law/jurisdictions/"/>
      <owl:imports rdf:resource="http://spec.edmcouncil.org/fibo/red/fnd/accounting/currency-amount/"/>
      <owl:imports rdf:resource="http://spec.edmcouncil.org/fibo/red/fnd/utilities/business-facing-types/"/>
   </owl:Ontology>


  <!--
    ///////////////////////////////////////////////////////////////////////////////////////
    //
    // Datatypes
    //
    ///////////////////////////////////////////////////////////////////////////////////////
    -->



  <!--
    ///////////////////////////////////////////////////////////////////////////////////////
    //
    // Object Properties
    //
    ///////////////////////////////////////////////////////////////////////////////////////
    -->


<owl:ObjectProperty rdf:about="&fibo-be-corp-corp;incorporatedCompanyHasIssuedCapital">
      <rdfs:label>incorporated company has issued capital</rdfs:label>
      <skos:definition>The amount of equity in the company, which has been issued in the form of shares (either publicly traded or privately held).</skos:definition>
      <rdfs:subPropertyOf rdf:resource="&fibo-be-corp-corp;hasIssuedCapital"/>
      <rdfs:domain rdf:resource="&fibo-be-corp-corp;IncorporatedCompany"/>
      <rdfs:range rdf:resource="&fibo-fnd-acc-cur;MonetaryAmount"/>
   </owl:ObjectProperty>

   <owl:ObjectProperty rdf:about="&fibo-be-corp-corp;incorporatedCompanyHasNominalCapital">
      <rdfs:label>incorporated company has nominal capital</rdfs:label>
      <skos:definition>The total amount of capital which the company is authorized to issue as equity in the form of shares, according to the company's legal documentation (Memorandum and Articles, or equivalent).</skos:definition>
      <rdfs:subPropertyOf rdf:resource="&fibo-be-corp-corp;hasNominalCapital"/>
      <rdfs:domain rdf:resource="&fibo-be-corp-corp;IncorporatedCompany"/>
      <rdfs:range rdf:resource="&fibo-fnd-acc-cur;MonetaryAmount"/>
   </owl:ObjectProperty>

   <owl:ObjectProperty rdf:about="&fibo-be-corp-corp;governedByBoardAgreement">
      <rdfs:label>governed by board agreement</rdfs:label>
      <skos:definition>The agreement which covers the relationships among the Board Members and between them and the Corporation as a legal entity.</skos:definition>
      <rdfs:subPropertyOf rdf:resource="&fibo-be-le-fbo;formallyConstitutedOrganizationIsGovernedBy"/>
      <rdfs:domain rdf:resource="&fibo-be-corp-corp;IncorporatedCompany"/>
      <rdfs:range rdf:resource="&fibo-be-corp-corp;BoardAgreement"/>
   </owl:ObjectProperty>

   <owl:ObjectProperty rdf:about="&fibo-be-corp-corp;hasIssuedCapital">
      <rdfs:label>has issued capital</rdfs:label>
      <skos:definition>The total of a companys shares that are held by shareholders. A company can, at any time, issue new shares up to the full amount of authorized share capital.</skos:definition>
      <rdfs:subPropertyOf rdf:resource="&fibo-be-corp-corp;hasNominalCapital"/>
      <rdfs:domain rdf:resource="&fibo-fnd-rel-rel;Thing"/>
      <rdfs:range rdf:resource="&fibo-fnd-acc-cur;MonetaryAmount"/>
   </owl:ObjectProperty>

   <owl:ObjectProperty rdf:about="&fibo-be-corp-corp;hasNominalCapital">
      <rdfs:label>has nominal capital</rdfs:label>
      <skos:definition>Nominal capital is an alternate term for authorized share capital. The maximum value of securities that a company can legally issue. This number is specified in the memorandum of association (or articles of incorporation in the US) when a company is incorporated, but can be changed later with shareholders approval. Authorized share capital may be divided into (1) Issued capital - par value of the shares actually issued, (2) Paid up capital - money received from the shareholders in exchange for shares, and (3) Uncalled capital - money remaining unpaid by the shareholders for the shares they have bought.</skos:definition>
      <rdfs:domain rdf:resource="&fibo-fnd-rel-rel;Thing"/>
      <rdfs:range rdf:resource="&fibo-fnd-acc-cur;MonetaryAmount"/>
   </owl:ObjectProperty>

   <owl:ObjectProperty rdf:about="&fibo-be-corp-corp;allocatedUnder">
      <rdfs:label>allocated under</rdfs:label>
      <skos:definition>The jurisdiction under which the registration code is allocated.</skos:definition>
      <rdfs:subPropertyOf rdf:resource="&fibo-fnd-rel-rel;isGoverneBy"/>
      <rdfs:domain rdf:resource="&fibo-be-corp-corp;CompanyRegistrationCode"/>
      <rdfs:range rdf:resource="&fibo-fnd-law-jur;Jurisdiction"/>
   </owl:ObjectProperty>

   <owl:ObjectProperty rdf:about="&fibo-be-corp-corp;hasRegistrationCode">
      <rdfs:label>has registration code</rdfs:label>
      <skos:definition>The official registration number of the incorporated company in the Jurisdiction in which it is registered.</skos:definition>
      <rdfs:subPropertyOf rdf:resource="&fibo-fnd-rel-rel;isIdentifiedBy"/>
      <rdfs:domain rdf:resource="&fibo-be-corp-corp;IncorporatedCompany"/>
      <rdfs:range rdf:resource="&fibo-be-corp-corp;CompanyRegistrationCode"/>
   </owl:ObjectProperty>


  <!--
    ///////////////////////////////////////////////////////////////////////////////////////
    //
    // Data Properties
    //
    ///////////////////////////////////////////////////////////////////////////////////////
    -->


<owl:DatatypeProperty rdf:about="&fibo-be-corp-corp;hasDateOfIncorporation">
      <rdfs:label>has date of incorporation</rdfs:label>
      <skos:definition>The date of formation of the company. This is identified as the formal date of registration in company registration documents.</skos:definition>
      <rdfs:range rdf:resource="http://www.w3.org/2001/XMLSchema#date"/>
   </owl:DatatypeProperty>

   <owl:DatatypeProperty rdf:about="&fibo-be-corp-corp;hasDateOfRegistration">
      <rdfs:label>has date of registration</rdfs:label>
      <skos:definition>Date at which the corporation is registered in some jurisdiction for regulatory and / or for tax purposes.</skos:definition>
      <rdfs:range rdf:resource="http://www.w3.org/2001/XMLSchema#date"/>
   </owl:DatatypeProperty>

   <owl:DatatypeProperty rdf:about="&fibo-be-corp-corp;hasLegalFormAbbreviation">
      <rdfs:label>has legal form abbreviation</rdfs:label>
      <skos:definition>The precise form of the incorporated company as defined in the jurisdiction in which it is registered, for example Ltd, PLC, Corp.</skos:definition>
      <rdfs:range rdf:resource="&fibo-fnd-utl-bt;text"/>
   </owl:DatatypeProperty>


  <!--
    ///////////////////////////////////////////////////////////////////////////////////////
    //
    // Annotation Properties
    //
    ///////////////////////////////////////////////////////////////////////////////////////
    -->



  <!--
    ///////////////////////////////////////////////////////////////////////////////////////
    //
    // Classes
    //
    ///////////////////////////////////////////////////////////////////////////////////////
    -->


<owl:Class rdf:about="&fibo-be-corp-corp;BoardAgreement">
      <rdfs:label>board agreement</rdfs:label>
      <skos:definition>The agreement between members of the Board of the Company.</skos:definition>
      <rdfs:subClassOf rdf:resource="&fibo-be-le-fbo;OrganizationCoveringAgreement"/>
   </owl:Class>

   <owl:Class rdf:about="&fibo-be-corp-corp;JointStockCompany">
      <rdfs:label>joint stock company</rdfs:label>
      <skos:definition>A joint stock company (JSC) is a type of business entity: it is a type of corporation or partnership between two companies. Certificates of ownership (or stocks) are issued by the company in return for each contribution, and the shareholders are free to transfer their ownership interest at any time by selling their stockholding to others.</skos:definition>
      <rdfs:subClassOf rdf:resource="&fibo-be-corp-corp;IncorporatedCompany"/>
   </owl:Class>

   <owl:Class rdf:about="&fibo-be-corp-corp;PrivatelyHeldCompany">
      <rdfs:label>privately held company</rdfs:label>
      <skos:definition>A company whose shares are held privately, usually by the directors or their relatives and associates.</skos:definition>
   </owl:Class>

   <owl:Class rdf:about="&fibo-be-corp-corp;PubliclyHeldCompany">
      <rdfs:label>publicly held company</rdfs:label>
      <skos:definition>A company whose shares are traded and held publicly.</skos:definition>
   </owl:Class>

   <owl:Class rdf:about="&fibo-be-corp-corp;CompanyRegistrationCode">
      <rdfs:label>company registration code</rdfs:label>
      <skos:definition>A code which is officially allocated under a jurisdiction in which a company is incorporated, and which is used within that jurisdiction to identify the company. This usually has to be included in official stationery and must always be publicly available.</skos:definition>
      <rdfs:subClassOf rdf:resource="&fibo-fnd-info-sch;RegistrationCode"/>
      <rdfs:subClassOf rdf:resource="&fibo-be-le-fbo;OrganizationIdentificationCode"/>
   </owl:Class>

   <owl:Class rdf:about="&fibo-be-corp-corp;IncorporatedCompany">
      <rdfs:label>incorporated company</rdfs:label>
      <skos:definition>A company incorporated by the issue of shares.</skos:definition>
      <rdfs:subClassOf rdf:resource="&fibo-be-le-cb;BodyIncorporatedWithEquity"/>
   </owl:Class>


  <!--
    ///////////////////////////////////////////////////////////////////////////////////////
    //
    // Individuals
    //
    ///////////////////////////////////////////////////////////////////////////////////////
    -->


</rdf:RDF>