<?xml version="1.0" encoding="UTF-8"?>
  
<!DOCTYPE rdf:RDF [
    <!ENTITY fibo-be-fct-fun "http://spec.edmcouncil.org/fibo/red/be/functional-entities-ext/fund-entities/">
    <!ENTITY fibo-be-fct-spv "http://spec.edmcouncil.org/fibo/red/be/functional-entities-ext/spv/">
    <!ENTITY fibo-be-fct-fct "http://spec.edmcouncil.org/fibo/red/be/functional-entities/functional-entities/">
    <!ENTITY fibo-sec-sec-pls "http://spec.edmcouncil.org/fibo/red/sec/securities/pools/">
    <!ENTITY fibo-civ-fun-civ "http://spec.edmcouncil.org/fibo/red/civ/funds/civ/">
    <!ENTITY fibo-fnd-tim-tim "http://spec.edmcouncil.org/fibo/red/fnd/date-time/date-time/">
]>

<rdf:RDF xmlns:xsd="http://www.w3.org/2001/XMLSchema#"
         xmlns:sm="http://www.omg.org/techprocess/ab/SpecificationMetadata/"
         xmlns:xs="http://www.w3.org/2001/XMLSchema"
         xmlns:fibo-fnd-utl-av="http://www.omg.org/spec/EDMC-FIBO/FND/Utilities/AnnotationVocabulary/"
         xmlns:rdf="http://www.w3.org/1999/02/22-rdf-syntax-ns#"
         xmlns:rdfs="http://www.w3.org/2000/01/rdf-schema#"
         xmlns:owl="http://www.w3.org/2002/07/owl#"
         xmlns:skos="http://www.w3.org/2004/02/skos/core#"
         xmlns:dc="http://purl.org/dc/terms/"
         xml:base="http://spec.edmcouncil.org/fibo/red/be/functional-entities-ext/fund-entities/">

   <owl:Ontology rdf:about="http://spec.edmcouncil.org/fibo/red/be/functional-entities-ext/fund-entities/">
      <owl:imports rdf:resource="http://spec.edmcouncil.org/fibo/red/be/functional-entities-ext/spv/"/>
      <owl:imports rdf:resource="http://spec.edmcouncil.org/fibo/red/be/functional-entities/functional-entities/"/>
      <owl:imports rdf:resource="http://spec.edmcouncil.org/fibo/red/sec/securities/pools/"/>
      <owl:imports rdf:resource="http://spec.edmcouncil.org/fibo/red/civ/funds/civ/"/>
      <owl:imports rdf:resource="http://spec.edmcouncil.org/fibo/red/fnd/date-time/date-time/"/>
   </owl:Ontology>


  <!--
    ///////////////////////////////////////////////////////////////////////////////////////
    //
    // Datatypes
    //
    ///////////////////////////////////////////////////////////////////////////////////////
    -->



  <!--
    ///////////////////////////////////////////////////////////////////////////////////////
    //
    // Object Properties
    //
    ///////////////////////////////////////////////////////////////////////////////////////
    -->


<owl:ObjectProperty rdf:about="&fibo-be-fct-fun;holds">
      <rdfs:label>holds</rdfs:label>
      <skos:definition>The Funds Special Purpose Vehicle holds this Fund.</skos:definition>
      <rdfs:subPropertyOf rdf:resource="&fibo-sec-sec-pls;sPVHoldsPool"/>
      <rdfs:domain rdf:resource="&fibo-be-fct-fun;FundsSPV"/>
      <rdfs:range rdf:resource="&fibo-civ-fun-civ;Fund"/>
   </owl:ObjectProperty>


  <!--
    ///////////////////////////////////////////////////////////////////////////////////////
    //
    // Data Properties
    //
    ///////////////////////////////////////////////////////////////////////////////////////
    -->


<owl:DatatypeProperty rdf:about="&fibo-be-fct-fun;intendedLiquidationDate">
      <rdfs:label>intended liquidation date</rdfs:label>
      <skos:definition>Intended or scheduled fund closing date - date of final NAV.</skos:definition>
      <rdfs:range rdf:resource="&fibo-fnd-tim-tim;Date"/>
   </owl:DatatypeProperty>

   <owl:DatatypeProperty rdf:about="&fibo-be-fct-fun;purpose">
      <rdfs:label>purpose</rdfs:label>
      <skos:definition>The purpose for which the SPV is set up. In this case it is set up in order to create and embody an investment fund.</skos:definition>
      <rdfs:range rdf:resource="&fibo-be-fct-spv;SPVPurposeSelection"/>
   </owl:DatatypeProperty>


  <!--
    ///////////////////////////////////////////////////////////////////////////////////////
    //
    // Annotation Properties
    //
    ///////////////////////////////////////////////////////////////////////////////////////
    -->



  <!--
    ///////////////////////////////////////////////////////////////////////////////////////
    //
    // Classes
    //
    ///////////////////////////////////////////////////////////////////////////////////////
    -->


<owl:Class rdf:about="&fibo-be-fct-fun;FCP">
      <rdfs:label>f c p</rdfs:label>
      <skos:definition>A French fund vehicle type. Designation and definition needed.</skos:definition>
      <rdfs:subClassOf rdf:resource="&fibo-be-fct-fct;FunctionalBusinessEntity"/>
   </owl:Class>

   <owl:Class rdf:about="&fibo-be-fct-fun;FundsSPV">
      <rdfs:label>funds s p v</rdfs:label>
      <skos:definition>A Special Purpose Vehicle (SPV) set up specifically to create an investment fund. It is set up by a company or a group of companies for this purpose. The SPV is formed for a specific reason and exists for a specific period of time and is then disbanded.</skos:definition>
      <rdfs:subClassOf rdf:resource="&fibo-be-fct-spv;SpecialPurposeVehicle"/>
   </owl:Class>

   <owl:Class rdf:about="&fibo-be-fct-fun;SICAF">
      <rdfs:label>s i c a f</rdfs:label>
      <skos:definition>A French fund vehicle type. Designation and definition needed.</skos:definition>
   </owl:Class>

   <owl:Class rdf:about="&fibo-be-fct-fun;SICAV">
      <rdfs:label>s i c a v</rdfs:label>
      <skos:definition>Societe Collective a Capital Variable</skos:definition>
   </owl:Class>


  <!--
    ///////////////////////////////////////////////////////////////////////////////////////
    //
    // Individuals
    //
    ///////////////////////////////////////////////////////////////////////////////////////
    -->


</rdf:RDF>