<?xml version="1.0" encoding="UTF-8"?>
<!DOCTYPE rdf:RDF [
	<!ENTITY dct "http://purl.org/dc/terms/">
	<!ENTITY fibo-fbc-dae-crf "https://spec.edmcouncil.org/fibo/ontology/FBC/DebtAndEquities/CreditFacilities/">
	<!ENTITY fibo-fbc-dae-dbt "https://spec.edmcouncil.org/fibo/ontology/FBC/DebtAndEquities/Debt/">
	<!ENTITY fibo-fbc-fi-fi "https://spec.edmcouncil.org/fibo/ontology/FBC/FinancialInstruments/FinancialInstruments/">
	<!ENTITY fibo-fnd-acc-cur "https://spec.edmcouncil.org/fibo/ontology/FND/Accounting/CurrencyAmount/">
	<!ENTITY fibo-fnd-agr-ctr "https://spec.edmcouncil.org/fibo/ontology/FND/Agreements/Contracts/">
	<!ENTITY fibo-fnd-agrx-ele "https://spec.edmcouncil.org/fibo/ontology/FND/AgreementsExt/ContractElements/">
	<!ENTITY fibo-fnd-arr-doc "https://spec.edmcouncil.org/fibo/ontology/FND/Arrangements/Documents/">
	<!ENTITY fibo-fnd-dt-fd "https://spec.edmcouncil.org/fibo/ontology/FND/DatesAndTimes/FinancialDates/">
	<!ENTITY fibo-fnd-gao-obj "https://spec.edmcouncil.org/fibo/ontology/FND/GoalsAndObjectives/Objectives/">
	<!ENTITY fibo-fnd-pty-pty "https://spec.edmcouncil.org/fibo/ontology/FND/Parties/Parties/">
	<!ENTITY fibo-fnd-utl-av "https://spec.edmcouncil.org/fibo/ontology/FND/Utilities/AnnotationVocabulary/">
	<!ENTITY fibo-fnd-utl-val "https://spec.edmcouncil.org/fibo/ontology/FND/Utilities/Values/">
	<!ENTITY fibo-loan-ln-ln "https://spec.edmcouncil.org/fibo/ontology/LOAN/LoanContracts/LoanCore/">
	<!ENTITY fibo-loan-loan-gty "https://spec.edmcouncil.org/fibo/ontology/LOAN/Loans/LoansGuaranties/">
	<!ENTITY fibo-loan-loan-loan "https://spec.edmcouncil.org/fibo/ontology/LOAN/Loans/LoanBasicTerms/">
	<!ENTITY fibo-loan-loan-pty "https://spec.edmcouncil.org/fibo/ontology/LOAN/Loans/LoansParties/">
	<!ENTITY fibo-loan-tem-ph "https://spec.edmcouncil.org/fibo/ontology/LOAN/LoansTemporal/LoanPhases/">
	<!ENTITY owl "http://www.w3.org/2002/07/owl#">
	<!ENTITY rdf "http://www.w3.org/1999/02/22-rdf-syntax-ns#">
	<!ENTITY rdfs "http://www.w3.org/2000/01/rdf-schema#">
	<!ENTITY skos "http://www.w3.org/2004/02/skos/core#">
	<!ENTITY xsd "http://www.w3.org/2001/XMLSchema#">
]>
<rdf:RDF xml:base="https://spec.edmcouncil.org/fibo/ontology/LOAN/Loans/LoanBasicTerms/"
	xmlns:dct="http://purl.org/dc/terms/"
	xmlns:fibo-fbc-dae-crf="https://spec.edmcouncil.org/fibo/ontology/FBC/DebtAndEquities/CreditFacilities/"
	xmlns:fibo-fbc-dae-dbt="https://spec.edmcouncil.org/fibo/ontology/FBC/DebtAndEquities/Debt/"
	xmlns:fibo-fbc-fi-fi="https://spec.edmcouncil.org/fibo/ontology/FBC/FinancialInstruments/FinancialInstruments/"
	xmlns:fibo-fnd-acc-cur="https://spec.edmcouncil.org/fibo/ontology/FND/Accounting/CurrencyAmount/"
	xmlns:fibo-fnd-agr-ctr="https://spec.edmcouncil.org/fibo/ontology/FND/Agreements/Contracts/"
	xmlns:fibo-fnd-agrx-ele="https://spec.edmcouncil.org/fibo/ontology/FND/AgreementsExt/ContractElements/"
	xmlns:fibo-fnd-arr-doc="https://spec.edmcouncil.org/fibo/ontology/FND/Arrangements/Documents/"
	xmlns:fibo-fnd-dt-fd="https://spec.edmcouncil.org/fibo/ontology/FND/DatesAndTimes/FinancialDates/"
	xmlns:fibo-fnd-gao-obj="https://spec.edmcouncil.org/fibo/ontology/FND/GoalsAndObjectives/Objectives/"
	xmlns:fibo-fnd-pty-pty="https://spec.edmcouncil.org/fibo/ontology/FND/Parties/Parties/"
	xmlns:fibo-fnd-utl-av="https://spec.edmcouncil.org/fibo/ontology/FND/Utilities/AnnotationVocabulary/"
	xmlns:fibo-fnd-utl-val="https://spec.edmcouncil.org/fibo/ontology/FND/Utilities/Values/"
	xmlns:fibo-loan-ln-ln="https://spec.edmcouncil.org/fibo/ontology/LOAN/LoanContracts/LoanCore/"
	xmlns:fibo-loan-loan-gty="https://spec.edmcouncil.org/fibo/ontology/LOAN/Loans/LoansGuaranties/"
	xmlns:fibo-loan-loan-loan="https://spec.edmcouncil.org/fibo/ontology/LOAN/Loans/LoanBasicTerms/"
	xmlns:fibo-loan-loan-pty="https://spec.edmcouncil.org/fibo/ontology/LOAN/Loans/LoansParties/"
	xmlns:fibo-loan-tem-ph="https://spec.edmcouncil.org/fibo/ontology/LOAN/LoansTemporal/LoanPhases/"
	xmlns:owl="http://www.w3.org/2002/07/owl#"
	xmlns:rdf="http://www.w3.org/1999/02/22-rdf-syntax-ns#"
	xmlns:rdfs="http://www.w3.org/2000/01/rdf-schema#"
	xmlns:skos="http://www.w3.org/2004/02/skos/core#"
	xmlns:xsd="http://www.w3.org/2001/XMLSchema#">
	
	<owl:Ontology rdf:about="https://spec.edmcouncil.org/fibo/ontology/LOAN/Loans/LoanBasicTerms/">
		<rdfs:label xml:lang="en">LoanBasicTerms</rdfs:label>
		<dct:abstract>This is the core ontology for loans concepts. These include loan purposes, loan payment terms and parties.</dct:abstract>
		<owl:imports rdf:resource="https://spec.edmcouncil.org/fibo/ontology/DER/CreditDerivatives/CreditDefaultSwaps/"/>
		<owl:imports rdf:resource="https://spec.edmcouncil.org/fibo/ontology/FBC/DebtAndEquities/CreditFacilities/"/>
		<owl:imports rdf:resource="https://spec.edmcouncil.org/fibo/ontology/FBC/DebtAndEquities/Debt/"/>
		<owl:imports rdf:resource="https://spec.edmcouncil.org/fibo/ontology/FBC/FinancialInstruments/FinancialInstruments/"/>
		<owl:imports rdf:resource="https://spec.edmcouncil.org/fibo/ontology/FND/Accounting/CurrencyAmount/"/>
		<owl:imports rdf:resource="https://spec.edmcouncil.org/fibo/ontology/FND/Agreements/Contracts/"/>
		<owl:imports rdf:resource="https://spec.edmcouncil.org/fibo/ontology/FND/AgreementsExt/ContractElements/"/>
		<owl:imports rdf:resource="https://spec.edmcouncil.org/fibo/ontology/FND/Arrangements/Documents/"/>
		<owl:imports rdf:resource="https://spec.edmcouncil.org/fibo/ontology/FND/DatesAndTimes/FinancialDates/"/>
		<owl:imports rdf:resource="https://spec.edmcouncil.org/fibo/ontology/FND/GoalsAndObjectives/Objectives/"/>
		<owl:imports rdf:resource="https://spec.edmcouncil.org/fibo/ontology/FND/Parties/Parties/"/>
		<owl:imports rdf:resource="https://spec.edmcouncil.org/fibo/ontology/FND/Relations/Relations/"/>
		<owl:imports rdf:resource="https://spec.edmcouncil.org/fibo/ontology/FND/Utilities/AnnotationVocabulary/"/>
		<owl:imports rdf:resource="https://spec.edmcouncil.org/fibo/ontology/FND/Utilities/Values/"/>
		<owl:imports rdf:resource="https://spec.edmcouncil.org/fibo/ontology/IND/InterestRates/InterestRates/"/>
		<owl:imports rdf:resource="https://spec.edmcouncil.org/fibo/ontology/IND/MarketIndices/BasketIndices/"/>
		<owl:imports rdf:resource="https://spec.edmcouncil.org/fibo/ontology/LOAN/LoanContracts/LoanCore/"/>
		<owl:imports rdf:resource="https://spec.edmcouncil.org/fibo/ontology/LOAN/Loans/LoansGuaranties/"/>
		<owl:imports rdf:resource="https://spec.edmcouncil.org/fibo/ontology/LOAN/Loans/LoansParties/"/>
		<owl:imports rdf:resource="https://spec.edmcouncil.org/fibo/ontology/LOAN/LoansTemporal/LoanPhases/"/>
		<owl:versionIRI rdf:resource="https://spec.edmcouncil.org/fibo/ontology/LOAN/Loans/LoanBasicTerms/"/>
		<fibo-fnd-utl-av:hasMaturityLevel rdf:resource="&fibo-fnd-utl-av;Provisional"/>
	</owl:Ontology>
	
	<owl:Class rdf:about="&fibo-fbc-dae-crf;CreditFacilityLoanTranche">
		<rdfs:subClassOf>
			<owl:Restriction>
				<owl:onProperty rdf:resource="&fibo-fbc-dae-crf;issuedAs"/>
				<owl:someValuesFrom rdf:resource="&fibo-loan-loan-loan;LoanDrawdown"/>
			</owl:Restriction>
		</rdfs:subClassOf>
	</owl:Class>
	
	<owl:Class rdf:about="&fibo-loan-ln-ln;Loan">
		<rdfs:subClassOf>
			<owl:Restriction>
				<owl:onProperty rdf:resource="&fibo-fnd-agr-ctr;definesTermsFor"/>
				<owl:someValuesFrom rdf:resource="&fibo-loan-loan-loan;LoanDrawdown"/>
			</owl:Restriction>
		</rdfs:subClassOf>
	</owl:Class>
	
	<owl:Class rdf:about="&fibo-loan-loan-loan;LoanDrawdown">
		<rdfs:subClassOf rdf:resource="&fibo-fbc-dae-dbt;Debt"/>
		<rdfs:subClassOf>
			<owl:Restriction>
				<owl:onProperty rdf:resource="&fibo-loan-loan-gty;guaranteedBy"/>
				<owl:allValuesFrom rdf:resource="&fibo-loan-loan-gty;LoanGuarantor"/>
			</owl:Restriction>
		</rdfs:subClassOf>
		<rdfs:subClassOf>
			<owl:Restriction>
				<owl:onProperty rdf:resource="&fibo-loan-loan-loan;loanSubsidyAmount"/>
				<owl:onClass rdf:resource="&fibo-fnd-acc-cur;MonetaryAmount"/>
				<owl:maxQualifiedCardinality rdf:datatype="&xsd;nonNegativeInteger">1</owl:maxQualifiedCardinality>
			</owl:Restriction>
		</rdfs:subClassOf>
		<rdfs:subClassOf>
			<owl:Restriction>
				<owl:onProperty rdf:resource="&fibo-fbc-fi-fi;hasTimeToMaturity"/>
				<owl:onClass rdf:resource="&fibo-fnd-dt-fd;ExplicitDuration"/>
				<owl:maxQualifiedCardinality rdf:datatype="&xsd;nonNegativeInteger">1</owl:maxQualifiedCardinality>
			</owl:Restriction>
		</rdfs:subClassOf>
		<rdfs:subClassOf>
			<owl:Restriction>
				<owl:onProperty rdf:resource="&fibo-fbc-dae-dbt;isCollateralizedBy"/>
				<owl:onClass rdf:resource="&fibo-fbc-dae-dbt;Collateral"/>
				<owl:minQualifiedCardinality rdf:datatype="&xsd;nonNegativeInteger">0</owl:minQualifiedCardinality>
			</owl:Restriction>
		</rdfs:subClassOf>
		<rdfs:subClassOf>
			<owl:Restriction>
				<owl:onProperty rdf:resource="&fibo-fbc-dae-dbt;hasBorrower"/>
				<owl:someValuesFrom rdf:resource="&fibo-fbc-dae-dbt;Borrower"/>
			</owl:Restriction>
		</rdfs:subClassOf>
		<rdfs:subClassOf>
			<owl:Restriction>
				<owl:onProperty rdf:resource="&fibo-fbc-dae-dbt;hasLender"/>
				<owl:someValuesFrom rdf:resource="&fibo-fbc-dae-dbt;Lender"/>
			</owl:Restriction>
		</rdfs:subClassOf>
		<rdfs:subClassOf>
			<owl:Restriction>
				<owl:onProperty rdf:resource="&fibo-fbc-fi-fi;hasTimeToMaturity"/>
				<owl:someValuesFrom rdf:resource="&fibo-fnd-dt-fd;ExplicitDuration"/>
			</owl:Restriction>
		</rdfs:subClassOf>
		<rdfs:subClassOf>
			<owl:Restriction>
				<owl:onProperty rdf:resource="&fibo-fnd-agr-ctr;hasContractualElement"/>
				<owl:someValuesFrom rdf:resource="&fibo-fbc-dae-dbt;DebtTerms"/>
			</owl:Restriction>
		</rdfs:subClassOf>
		<rdfs:subClassOf>
			<owl:Restriction>
				<owl:onProperty rdf:resource="&fibo-loan-loan-loan;drawnDownBy"/>
				<owl:someValuesFrom rdf:resource="&fibo-fbc-dae-dbt;Borrower"/>
			</owl:Restriction>
		</rdfs:subClassOf>
		<rdfs:subClassOf>
			<owl:Restriction>
				<owl:onProperty rdf:resource="&fibo-loan-loan-pty;hasLoanThirdParty"/>
				<owl:someValuesFrom rdf:resource="&fibo-loan-loan-pty;LoanThirdParty"/>
			</owl:Restriction>
		</rdfs:subClassOf>
		<rdfs:subClassOf>
			<owl:Restriction>
				<owl:onProperty rdf:resource="&fibo-loan-loan-pty;originatedBy"/>
				<owl:someValuesFrom rdf:resource="&fibo-loan-loan-loan;LoanOriginator"/>
			</owl:Restriction>
		</rdfs:subClassOf>
		<rdfs:subClassOf>
			<owl:Restriction>
				<owl:onProperty rdf:resource="&fibo-loan-loan-pty;servicedBy"/>
				<owl:someValuesFrom rdf:resource="&fibo-loan-loan-pty;LoanServicer"/>
			</owl:Restriction>
		</rdfs:subClassOf>
		<rdfs:label xml:lang="en">loan drawdown</rdfs:label>
		<skos:definition xml:lang="en">An amount of money, drawn down by one party (the borrower) from a credit tranche made available by another party (the lender) at a specific point in time. Formal terms for the loan are defined in a Loan Contract.</skos:definition>
		<fibo-fnd-utl-av:explanatoryNote xml:lang="en">This is not the amount owed at a specific point in time (that is the Loan Balance) but rather the amount drawn down as a loan. The balance of the loan changes over time as principal is paid off, and the balance of monies between the lender and the borrower is further impacted by interest payments, interest due and fees.</fibo-fnd-utl-av:explanatoryNote>
	</owl:Class>
	
	<owl:Class rdf:about="&fibo-loan-loan-loan;LoanOriginator">
		<rdfs:subClassOf rdf:resource="&fibo-fnd-pty-pty;PartyInRole"/>
		<rdfs:label xml:lang="en">loan originator</rdfs:label>
		<skos:definition xml:lang="en">The party which finds the lender for the loan, for the borrower.</skos:definition>
		<fibo-fnd-utl-av:explanatoryNote xml:lang="en">Similar to mortgages: the originator may be a bank but the person able to lend the money may be some other party. In other instances the originator will become the lender.</fibo-fnd-utl-av:explanatoryNote>
	</owl:Class>
	
	<owl:Class rdf:about="&fibo-loan-loan-loan;LoanParty">
		<rdfs:subClassOf rdf:resource="&fibo-fnd-agr-ctr;ContractParty"/>
		<rdfs:label xml:lang="en">loan party</rdfs:label>
		<skos:definition xml:lang="en">A Party to the Loan.</skos:definition>
		<skos:editorialNote xml:lang="en">This covers the principals to the Loan contract (Loan Borrower and Loan Lender) as well as third parties, including Loan Originator. Transformation notes: In the PoC SDM the sub-classes of Loan Third Party will not be articulated as separate parties but defined via a selection list under &quot;Loan Party&quot; or &quot;Loan Third Party&quot;.</skos:editorialNote>
	</owl:Class>
	
	<owl:Class rdf:about="&fibo-loan-loan-loan;LoanRetainedAmount">
		<rdfs:subClassOf rdf:resource="&fibo-fnd-acc-cur;MonetaryAmount"/>
		<rdfs:label xml:lang="en">loan retained amount</rdfs:label>
		<skos:definition xml:lang="en">Retained amount, an amount the Issuer will be obliged to fund to the borrower at a later date, for example construction deposit.</skos:definition>
		<skos:editorialNote xml:lang="en">This is a monetary amount by descent from the Monetary Amount term in the taxonomy of kinds of amount. Hence it does not have a monetary amount attribute because it is one.</skos:editorialNote>
	</owl:Class>
	
	<owl:ObjectProperty rdf:about="&fibo-loan-loan-loan;accepts">
		<rdfs:label xml:lang="en">accepts</rdfs:label>
		<rdfs:domain rdf:resource="&fibo-fbc-dae-dbt;Borrower"/>
		<rdfs:range rdf:resource="&fibo-loan-ln-ln;CommitmentToRepay"/>
	</owl:ObjectProperty>
	
	<owl:ObjectProperty rdf:about="&fibo-loan-loan-loan;borrows">
		<rdfs:label xml:lang="en">borrows</rdfs:label>
		<rdfs:domain rdf:resource="&fibo-fbc-dae-dbt;Borrower"/>
		<rdfs:range rdf:resource="&fibo-loan-loan-loan;LoanDrawdown"/>
	</owl:ObjectProperty>
	
	<owl:DatatypeProperty rdf:about="&fibo-loan-loan-loan;buydownExists">
		<rdfs:label xml:lang="en">buydown exists</rdfs:label>
		<rdfs:domain rdf:resource="&fibo-loan-loan-loan;LoanDrawdown"/>
		<rdfs:range rdf:resource="&xsd;boolean"/>
		<skos:definition xml:lang="en">Whether a third party (usually a builder) is making payments to subsize a borrower.</skos:definition>
	</owl:DatatypeProperty>
	
	<owl:DatatypeProperty rdf:about="&fibo-loan-loan-loan;drawDownDate">
		<rdfs:label xml:lang="en">draw down date</rdfs:label>
		<rdfs:domain rdf:resource="&fibo-loan-loan-loan;LoanDrawdown"/>
		<skos:definition xml:lang="en">The date on which the funds are drawn down, that define the start of the loan.</skos:definition>
	</owl:DatatypeProperty>
	
	<owl:ObjectProperty rdf:about="&fibo-loan-loan-loan;drawnDownBy">
		<rdfs:subPropertyOf rdf:resource="&fibo-fbc-dae-dbt;hasBorrower"/>
		<rdfs:label xml:lang="en">drawn down by</rdfs:label>
		<rdfs:domain rdf:resource="&fibo-loan-loan-loan;LoanDrawdown"/>
		<rdfs:range rdf:resource="&fibo-fbc-dae-dbt;Borrower"/>
		<owl:inverseOf rdf:resource="&fibo-loan-loan-loan;borrows"/>
	</owl:ObjectProperty>
	
	<owl:DatatypeProperty rdf:about="&fibo-loan-loan-loan;escrowApplicable">
		<rdfs:label xml:lang="en">escrow applicable</rdfs:label>
		<rdfs:domain rdf:resource="&fibo-loan-ln-ln;Loan"/>
		<rdfs:range rdf:resource="&xsd;boolean"/>
		<skos:definition xml:lang="en">Whether the servicer is contractually responsible for maintaining an escrow against the account for payment of txes and insurance.</skos:definition>
	</owl:DatatypeProperty>
	
	<owl:DatatypeProperty rdf:about="&fibo-loan-loan-loan;loanGuarantorType">
		<rdfs:label xml:lang="en">loan guarantor type</rdfs:label>
		<rdfs:domain rdf:resource="&fibo-loan-loan-loan;LoanDrawdown"/>
		<skos:definition xml:lang="en">The type of guarantee provider, if applicable. Actiojn: Move down th eGuaranteed Loan.</skos:definition>
	</owl:DatatypeProperty>
	
	<owl:ObjectProperty rdf:about="&fibo-loan-loan-loan;loanMaximumAllowedBalance">
		<rdfs:label xml:lang="en">loan maximum allowed balance</rdfs:label>
		<rdfs:domain rdf:resource="&fibo-loan-ln-ln;Loan"/>
		<rdfs:range rdf:resource="&fibo-fnd-acc-cur;MonetaryAmount"/>
		<skos:definition xml:lang="en">Maximum balance - For loans with flexible re-draw facilities, the maximum loan amount that could potentially be outstanding</skos:definition>
	</owl:ObjectProperty>
	
	<owl:ObjectProperty rdf:about="&fibo-loan-loan-loan;loanOriginalAdvanceAmount">
		<rdfs:label xml:lang="en">loan original advance amount</rdfs:label>
		<rdfs:domain rdf:resource="&fibo-loan-ln-ln;Loan"/>
		<rdfs:range rdf:resource="&fibo-fnd-acc-cur;MonetaryAmount"/>
		<skos:definition xml:lang="en">The Original Balance of the loan, that is the amount advanced under this loan. Further notes: PoC workings: Original balance (inclusive of fees)</skos:definition>
	</owl:ObjectProperty>
	
	<owl:DatatypeProperty rdf:about="&fibo-loan-loan-loan;loanOriginalAdvanceDate">
		<rdfs:label xml:lang="en">loan original advance date</rdfs:label>
		<rdfs:domain rdf:resource="&fibo-loan-loan-loan;LoanDrawdown"/>
		<skos:definition xml:lang="en">Loan origination date, that is the date of original loan advance.</skos:definition>
	</owl:DatatypeProperty>
	
	<owl:ObjectProperty rdf:about="&fibo-loan-loan-loan;loanRetainedAmount">
		<rdfs:label xml:lang="en">loan retained amount</rdfs:label>
		<rdfs:domain rdf:resource="&fibo-loan-ln-ln;Loan"/>
		<rdfs:range rdf:resource="&fibo-fnd-acc-cur;MonetaryAmount"/>
		<skos:definition xml:lang="en">Retained amount, this is an amount the Issuer will be obliged to fund to the borrower at a later date, for example construction deposit.</skos:definition>
	</owl:ObjectProperty>
	
	<owl:DatatypeProperty rdf:about="&fibo-loan-loan-loan;loanRetainedAmountDate">
		<rdfs:label xml:lang="en">loan retained amount date</rdfs:label>
		<rdfs:domain rdf:resource="&fibo-loan-ln-ln;Loan"/>
		<skos:definition xml:lang="en">Date when the retained amount is to be drawn by.</skos:definition>
	</owl:DatatypeProperty>
	
	<owl:ObjectProperty rdf:about="&fibo-loan-loan-loan;loanSubsidyAmount">
		<rdfs:label xml:lang="en">loan subsidy amount</rdfs:label>
		<rdfs:domain rdf:resource="&fibo-loan-loan-loan;LoanDrawdown"/>
		<rdfs:range rdf:resource="&fibo-fnd-acc-cur;MonetaryAmount"/>
		<skos:definition xml:lang="en">Loan Subsidy Received - Amount of subsidy received from government by borrower.</skos:definition>
	</owl:ObjectProperty>
	
	<owl:DatatypeProperty rdf:about="&fibo-loan-loan-loan;recourseLoan">
		<rdfs:label xml:lang="en">recourse loan</rdfs:label>
		<rdfs:domain rdf:resource="&fibo-loan-loan-loan;LoanDrawdown"/>
		<rdfs:range rdf:resource="&xsd;boolean"/>
		<skos:definition xml:lang="en">The only way you get the money back in the event of default is the security. Recourse is where you still have the opportunity to go back to the borrower for the rest of the money.</skos:definition>
	</owl:DatatypeProperty>
	
	<owl:ObjectProperty rdf:about="&fibo-loan-loan-loan;retainedUntil">
		<rdfs:label xml:lang="en">retained until</rdfs:label>
		<rdfs:domain rdf:resource="&fibo-loan-loan-loan;LoanRetainedAmount"/>
		<rdfs:range rdf:resource="&fibo-fnd-dt-fd;Date"/>
		<skos:definition xml:lang="en">Date when the retained amount is to be drawn by.</skos:definition>
	</owl:ObjectProperty>
	
	<owl:DatatypeProperty rdf:about="&fibo-loan-loan-loan;secured">
		<rdfs:label xml:lang="en">secured</rdfs:label>
		<rdfs:domain rdf:resource="&fibo-loan-loan-loan;LoanDrawdown"/>
		<rdfs:range rdf:resource="&xsd;boolean"/>
		<skos:definition xml:lang="en">Whether the loan is secured. Further Details: All loans are either secured or unsecured All secured loans are secured by some asset or some guaranty Guaranties have various forms. Guaranties have a guarantor. The guarantor may or may not elect to introduce some collateral of their own. Guarantor may or may not be Co-borrower.</skos:definition>
	</owl:DatatypeProperty>
	
	<owl:ObjectProperty rdf:about="&fibo-loan-loan-loan;spread">
		<rdfs:label xml:lang="en">spread</rdfs:label>
		<rdfs:domain rdf:resource="&fibo-fbc-dae-dbt;InterestPaymentTerms"/>
		<rdfs:range rdf:resource="&fibo-fnd-utl-val;PercentageValue"/>
		<skos:definition xml:lang="en">The percentage of interest added to the base rate.</skos:definition>
	</owl:ObjectProperty>
	
	<owl:DatatypeProperty rdf:about="&fibo-loan-loan-loan;subsidyPeriodEndDate">
		<rdfs:label xml:lang="en">subsidy period end date</rdfs:label>
		<rdfs:domain rdf:resource="&fibo-loan-loan-loan;LoanDrawdown"/>
		<skos:definition xml:lang="en">Subsidy Period - date at which subsidy period ends</skos:definition>
	</owl:DatatypeProperty>

</rdf:RDF>