<?xml version="1.0" encoding="UTF-8"?>
<!DOCTYPE rdf:RDF [
	<!ENTITY dct "http://purl.org/dc/terms/">
	<!ENTITY fibo-fbc-dae-crf "https://spec.edmcouncil.org/fibo/ontology/FBC/DebtAndEquities/CreditFacilities/">
	<!ENTITY fibo-fnd-acc-cur "https://spec.edmcouncil.org/fibo/ontology/FND/Accounting/CurrencyAmount/">
	<!ENTITY fibo-fnd-arr-cls "https://spec.edmcouncil.org/fibo/ontology/FND/Arrangements/ClassificationSchemes/">
	<!ENTITY fibo-fnd-plc-loc "https://spec.edmcouncil.org/fibo/ontology/FND/Places/Locations/">
	<!ENTITY fibo-fnd-utl-av "https://spec.edmcouncil.org/fibo/ontology/FND/Utilities/AnnotationVocabulary/">
	<!ENTITY fibo-loan-ln-ev "https://spec.edmcouncil.org/fibo/ontology/LOAN/LoanContracts/LoanEvents/">
	<!ENTITY fibo-loan-ln-ln "https://spec.edmcouncil.org/fibo/ontology/LOAN/LoanContracts/LoanCore/">
	<!ENTITY fibo-loan-loan-loan "https://spec.edmcouncil.org/fibo/ontology/LOAN/Loans/LoanBasicTerms/">
	<!ENTITY fibo-loan-typ-cl "https://spec.edmcouncil.org/fibo/ontology/LOAN/LoanTypes/ConstructionLoans/">
	<!ENTITY lcc-cr "https://www.omg.org/spec/LCC/Countries/CountryRepresentation/">
	<!ENTITY owl "http://www.w3.org/2002/07/owl#">
	<!ENTITY rdf "http://www.w3.org/1999/02/22-rdf-syntax-ns#">
	<!ENTITY rdfs "http://www.w3.org/2000/01/rdf-schema#">
	<!ENTITY skos "http://www.w3.org/2004/02/skos/core#">
	<!ENTITY sm "http://www.omg.org/techprocess/ab/SpecificationMetadata/">
	<!ENTITY xsd "http://www.w3.org/2001/XMLSchema#">
]>
<rdf:RDF xml:base="https://spec.edmcouncil.org/fibo/ontology/LOAN/LoanTypes/ConstructionLoans/"
	xmlns:dct="http://purl.org/dc/terms/"
	xmlns:fibo-fbc-dae-crf="https://spec.edmcouncil.org/fibo/ontology/FBC/DebtAndEquities/CreditFacilities/"
	xmlns:fibo-fnd-acc-cur="https://spec.edmcouncil.org/fibo/ontology/FND/Accounting/CurrencyAmount/"
	xmlns:fibo-fnd-arr-cls="https://spec.edmcouncil.org/fibo/ontology/FND/Arrangements/ClassificationSchemes/"
	xmlns:fibo-fnd-plc-loc="https://spec.edmcouncil.org/fibo/ontology/FND/Places/Locations/"
	xmlns:fibo-fnd-utl-av="https://spec.edmcouncil.org/fibo/ontology/FND/Utilities/AnnotationVocabulary/"
	xmlns:fibo-loan-ln-ev="https://spec.edmcouncil.org/fibo/ontology/LOAN/LoanContracts/LoanEvents/"
	xmlns:fibo-loan-ln-ln="https://spec.edmcouncil.org/fibo/ontology/LOAN/LoanContracts/LoanCore/"
	xmlns:fibo-loan-loan-loan="https://spec.edmcouncil.org/fibo/ontology/LOAN/Loans/LoanBasicTerms/"
	xmlns:fibo-loan-typ-cl="https://spec.edmcouncil.org/fibo/ontology/LOAN/LoanTypes/ConstructionLoans/"
	xmlns:lcc-cr="https://www.omg.org/spec/LCC/Countries/CountryRepresentation/"
	xmlns:owl="http://www.w3.org/2002/07/owl#"
	xmlns:rdf="http://www.w3.org/1999/02/22-rdf-syntax-ns#"
	xmlns:rdfs="http://www.w3.org/2000/01/rdf-schema#"
	xmlns:skos="http://www.w3.org/2004/02/skos/core#"
	xmlns:sm="http://www.omg.org/techprocess/ab/SpecificationMetadata/"
	xmlns:xsd="http://www.w3.org/2001/XMLSchema#">
	
	<owl:Ontology rdf:about="https://spec.edmcouncil.org/fibo/ontology/LOAN/LoanTypes/ConstructionLoans/">
		<rdfs:label xml:lang="en">ConstructionLoans</rdfs:label>
		<dct:abstract>Construction loans are loans in name only, in that the concept referred to as a construction loan is effectively a credit facility, with separate draw-downs (loans as defined in these ontologies) being enabled upon evidence of completion of agreed stages of the construction project, 
		Note that for completion this ontology will need to be extended with a number of project management concepts describing the parameters of the construction project that are referred to in the contract for this facility. Some basic project management terms such as milestones are already included but will need framing within more foundational concepts for project management.</dct:abstract>
		<sm:fileAbbreviation>fibo-loan-typ-cl</sm:fileAbbreviation>
		<owl:imports rdf:resource="https://spec.edmcouncil.org/fibo/ontology/FBC/DebtAndEquities/CreditFacilities/"/>
		<owl:imports rdf:resource="https://spec.edmcouncil.org/fibo/ontology/FND/Accounting/CurrencyAmount/"/>
		<owl:imports rdf:resource="https://spec.edmcouncil.org/fibo/ontology/FND/Arrangements/ClassificationSchemes/"/>
		<owl:imports rdf:resource="https://spec.edmcouncil.org/fibo/ontology/FND/Places/Locations/"/>
		<owl:imports rdf:resource="https://spec.edmcouncil.org/fibo/ontology/FND/Utilities/AnnotationVocabulary/"/>
		<owl:imports rdf:resource="https://spec.edmcouncil.org/fibo/ontology/LOAN/LoanContracts/LoanCore/"/>
		<owl:imports rdf:resource="https://spec.edmcouncil.org/fibo/ontology/LOAN/LoanContracts/LoanEvents/"/>
		<owl:imports rdf:resource="https://spec.edmcouncil.org/fibo/ontology/LOAN/Loans/LoanBasicTerms/"/>
		<owl:imports rdf:resource="https://www.omg.org/spec/LCC/Countries/CountryRepresentation/"/>
		<owl:versionIRI rdf:resource="https://spec.edmcouncil.org/fibo/ontology/LOAN/LoanTypes/ConstructionLoans/"/>
		<fibo-fnd-utl-av:hasMaturityLevel rdf:resource="&fibo-fnd-utl-av;Provisional"/>
	</owl:Ontology>
	
	<owl:Class rdf:about="&fibo-fnd-plc-loc;RealEstate">
		<rdfs:subClassOf>
			<owl:Restriction>
				<owl:onProperty rdf:resource="&lcc-cr;isClassifiedBy"/>
				<owl:someValuesFrom rdf:resource="&fibo-loan-typ-cl;ConstructionType"/>
			</owl:Restriction>
		</rdfs:subClassOf>
	</owl:Class>
	
	<owl:Class rdf:about="&fibo-loan-typ-cl;ConstructionLoan">
		<rdfs:subClassOf rdf:resource="&fibo-loan-ln-ln;Loan"/>
		<rdfs:label xml:lang="en">construction loan</rdfs:label>
		<skos:definition xml:lang="en">loan covering construction and development costs, secured by a mortgage on the property financed</skos:definition>
		<fibo-fnd-utl-av:synonym xml:lang="en">construction mortgage</fibo-fnd-utl-av:synonym>
	</owl:Class>
	
	<owl:Class rdf:about="&fibo-loan-typ-cl;ConstructionLoanContract">
		<rdfs:subClassOf rdf:resource="&fibo-fbc-dae-crf;CreditFacilityAgreement"/>
		<rdfs:subClassOf>
			<owl:Restriction>
				<owl:onProperty rdf:resource="&fibo-fbc-dae-crf;setsOutCommitmentTo"/>
				<owl:someValuesFrom rdf:resource="&fibo-loan-typ-cl;ConstructionLoanCreditFacilityTranche"/>
			</owl:Restriction>
		</rdfs:subClassOf>
		<rdfs:subClassOf>
			<owl:Restriction>
				<owl:onProperty rdf:resource="&fibo-loan-typ-cl;hasMilestoneTerm"/>
				<owl:someValuesFrom rdf:resource="&fibo-loan-typ-cl;ConstructionLoanMilestoneTermsSet"/>
			</owl:Restriction>
		</rdfs:subClassOf>
		<rdfs:label xml:lang="en">construction loan contract</rdfs:label>
	</owl:Class>
	
	<owl:Class rdf:about="&fibo-loan-typ-cl;ConstructionLoanCreditFacilityTranche">
		<rdfs:subClassOf rdf:resource="&fibo-fbc-dae-crf;CommittedCreditFacilityTranche"/>
		<rdfs:subClassOf>
			<owl:Restriction>
				<owl:onProperty rdf:resource="&fibo-fbc-dae-crf;issuedAs"/>
				<owl:someValuesFrom rdf:resource="&fibo-loan-typ-cl;ConstructionLoan"/>
			</owl:Restriction>
		</rdfs:subClassOf>
		<rdfs:label xml:lang="en">construction loan credit facility tranche</rdfs:label>
		<skos:definition xml:lang="en">A loan taken out for construction purposes. Further notes: These are a temporary loan. when the construction is finished then that loan is transformed to another loan, which would be a permanent loan. Information to follow on what the new permanent loan would be. Terms are adjusted in the new loan, since in construction loans the rates are significantly higher. This is an incentive to complete the construction works. Notes from PoC reviews, discussing Maximum Balance concept: In a Construction Loan you agree a maximum amount that you could draw. As you progress with the construction you continue to draw more and more. So you start with the minimum. Example: for purpose of construction of a house you could need to borrow up to 500K and the bank establishes the milestones at which certain amounts are made availalbe and can be drawn. For instance prior to start you might draw 10%, (50K); the next 50K would be available to draw only once the foundations are laid. And so on. Milestones may include &quot;Frame standing&quot; (for American-style frame based houses). Each stage requires inspection on behalf of the bank. So you are starting with no more than 10% (in this example) of what is allowable, and could arrive to the full 500K by the end of ths construction but it is not mandated that you arrive to that. What differentiates a Construction Loan is that there si a max amount specified and there are Milestones specified in which the amounts for each milestone can be advanced.</skos:definition>
	</owl:Class>
	
	<owl:Class rdf:about="&fibo-loan-typ-cl;ConstructionLoanMilestoneTermsSet">
		<rdfs:subClassOf rdf:resource="&fibo-fbc-dae-crf;LoanPrecedentConditions"/>
		<rdfs:label xml:lang="en">construction loan milestone terms set</rdfs:label>
		<skos:definition xml:lang="en">An agreed point at which an amount is advanced to the lender on completion of some pre-agreed scope of works on the construction.</skos:definition>
		<skos:editorialNote xml:lang="en">from review of a separate question, where we identified the need for this term:</skos:editorialNote>
	</owl:Class>
	
	<owl:Class rdf:about="&fibo-loan-typ-cl;ConstructionType">
		<rdfs:subClassOf rdf:resource="&fibo-fnd-arr-cls;Classifier"/>
		<rdfs:label>construction type</rdfs:label>
		<skos:definition>particular kind of construction</skos:definition>
	</owl:Class>
	
	<owl:NamedIndividual rdf:about="&fibo-loan-typ-cl;ConstructionType_Manufactured">
		<rdf:type rdf:resource="&fibo-loan-typ-cl;ConstructionType"/>
		<rdfs:label>manufactured</rdfs:label>
		<skos:definition>a factory-built dwelling built in compliance with the Federal Manufactured Home Construction and Safety Standards in effect at the time the home was manufactured as evidenced by the HUD label</skos:definition>
	</owl:NamedIndividual>
	
	<owl:NamedIndividual rdf:about="&fibo-loan-typ-cl;ConstructionType_MobileHome">
		<rdf:type rdf:resource="&fibo-loan-typ-cl;ConstructionType"/>
		<rdfs:label>mobile home</rdfs:label>
		<skos:definition>a dwelling unit constructed on a base frame which features wheels and axles to be used in transporting home from place to place</skos:definition>
		<fibo-fnd-utl-av:explanatoryNote>It does not meet HUD code.</fibo-fnd-utl-av:explanatoryNote>
	</owl:NamedIndividual>
	
	<owl:NamedIndividual rdf:about="&fibo-loan-typ-cl;ConstructionType_Modular">
		<rdf:type rdf:resource="&fibo-loan-typ-cl;ConstructionType"/>
		<rdfs:label>modular</rdfs:label>
		<skos:definition>a factory-built dwelling not on a permanent chassis</skos:definition>
	</owl:NamedIndividual>
	
	<owl:NamedIndividual rdf:about="&fibo-loan-typ-cl;ConstructionType_OnFrameModular">
		<rdf:type rdf:resource="&fibo-loan-typ-cl;ConstructionType"/>
		<rdfs:label>on frame modular</rdfs:label>
		<skos:definition>a factory built dwelling on a permanent chassis which does not have a HUD label</skos:definition>
	</owl:NamedIndividual>
	
	<owl:NamedIndividual rdf:about="&fibo-loan-typ-cl;ConstructionType_SiteBuilt">
		<rdf:type rdf:resource="&fibo-loan-typ-cl;ConstructionType"/>
		<rdfs:label>site built</rdfs:label>
		<skos:definition>describes construction process, indicating that most elements are created at the homes permanent site. May include some prefabricated components</skos:definition>
	</owl:NamedIndividual>
	
	<owl:ObjectProperty rdf:about="&fibo-loan-typ-cl;hasMaximumAllowedBalance">
		<rdfs:label xml:lang="en">has maximum allowed balance</rdfs:label>
		<rdfs:domain rdf:resource="&fibo-loan-typ-cl;ConstructionLoanContract"/>
		<rdfs:range rdf:resource="&fibo-fnd-acc-cur;MonetaryAmount"/>
		<skos:definition xml:lang="en">Maximum balance - For loans with flexible re-draw facilities, the maximum balance that could potentially be outstanding based on a credit limit</skos:definition>
	</owl:ObjectProperty>
	
	<owl:ObjectProperty rdf:about="&fibo-loan-typ-cl;hasMaximumAnticipatedBalance">
		<rdfs:label xml:lang="en">has maximum anticipated balance</rdfs:label>
		<rdfs:domain rdf:resource="&fibo-loan-typ-cl;ConstructionLoanCreditFacilityTranche"/>
		<rdfs:range rdf:resource="&fibo-fnd-acc-cur;MonetaryAmount"/>
		<skos:definition xml:lang="en">Maximum balance - For loans with flexible re-draw facilities, the maximum balance the borrower believes they might need, below the credit limit, for planning purposes</skos:definition>
	</owl:ObjectProperty>
	
	<owl:DatatypeProperty rdf:about="&fibo-loan-typ-cl;hasMilestoneDescription">
		<rdfs:label xml:lang="en">has milestone description</rdfs:label>
		<rdfs:domain rdf:resource="&fibo-loan-typ-cl;ConstructionLoanMilestoneTermsSet"/>
		<rdfs:range rdf:resource="&xsd;string"/>
		<skos:definition xml:lang="en">A textual description of the point at which it is legally recognized that the construction milestone has been reached.</skos:definition>
	</owl:DatatypeProperty>
	
	<owl:ObjectProperty rdf:about="&fibo-loan-typ-cl;hasMilestoneMaximumDrawdownAmount">
		<rdfs:label xml:lang="en">has milestone maximum drawdown amount</rdfs:label>
		<rdfs:domain rdf:resource="&fibo-loan-typ-cl;ConstructionLoanMilestoneTermsSet"/>
		<rdfs:range rdf:resource="&fibo-fnd-acc-cur;MonetaryAmount"/>
		<skos:definition xml:lang="en">The maximum amount of the loan that can be drawn by the Borrower on completion of this Milestone.</skos:definition>
	</owl:ObjectProperty>
	
	<owl:ObjectProperty rdf:about="&fibo-loan-typ-cl;hasMilestoneTerm">
		<rdfs:label xml:lang="en">has milestone term</rdfs:label>
		<rdfs:domain rdf:resource="&fibo-loan-typ-cl;ConstructionLoanContract"/>
		<rdfs:range rdf:resource="&fibo-loan-typ-cl;ConstructionLoanMilestoneTermsSet"/>
	</owl:ObjectProperty>

</rdf:RDF>