<?xml version="1.0" encoding="UTF-8"?>
<!DOCTYPE rdf:RDF [
	<!ENTITY dct "http://purl.org/dc/terms/">
	<!ENTITY fibo-fbc-dae-crf "https://spec.edmcouncil.org/fibo/FBC/DebtAndEquities/CreditFacilities/">
	<!ENTITY fibo-fbc-dae-dbt "https://spec.edmcouncil.org/fibo/FBC/DebtAndEquities/Debt/">
	<!ENTITY fibo-fnd-acc-cur "https://spec.edmcouncil.org/fibo/FND/Accounting/CurrencyAmount/">
	<!ENTITY fibo-fnd-utl-av "https://spec.edmcouncil.org/fibo/FND/Utilities/AnnotationVocabulary/">
	<!ENTITY fibo-loan-typ-cr "https://spec.edmcouncil.org/fibo/LOAN/LoanTypes/CreditProducts/">
	<!ENTITY owl "http://www.w3.org/2002/07/owl#">
	<!ENTITY rdf "http://www.w3.org/1999/02/22-rdf-syntax-ns#">
	<!ENTITY rdfs "http://www.w3.org/2000/01/rdf-schema#">
	<!ENTITY skos "http://www.w3.org/2004/02/skos/core#">
	<!ENTITY xsd "http://www.w3.org/2001/XMLSchema#">
]>
<rdf:RDF xml:base="https://spec.edmcouncil.org/fibo/LOAN/LoanTypes/CreditProducts/"
	xmlns:dct="http://purl.org/dc/terms/"
	xmlns:fibo-fbc-dae-crf="https://spec.edmcouncil.org/fibo/FBC/DebtAndEquities/CreditFacilities/"
	xmlns:fibo-fbc-dae-dbt="https://spec.edmcouncil.org/fibo/FBC/DebtAndEquities/Debt/"
	xmlns:fibo-fnd-acc-cur="https://spec.edmcouncil.org/fibo/FND/Accounting/CurrencyAmount/"
	xmlns:fibo-fnd-utl-av="https://spec.edmcouncil.org/fibo/FND/Utilities/AnnotationVocabulary/"
	xmlns:fibo-loan-typ-cr="https://spec.edmcouncil.org/fibo/LOAN/LoanTypes/CreditProducts/"
	xmlns:owl="http://www.w3.org/2002/07/owl#"
	xmlns:rdf="http://www.w3.org/1999/02/22-rdf-syntax-ns#"
	xmlns:rdfs="http://www.w3.org/2000/01/rdf-schema#"
	xmlns:skos="http://www.w3.org/2004/02/skos/core#"
	xmlns:xsd="http://www.w3.org/2001/XMLSchema#">
	
	<owl:Ontology rdf:about="https://spec.edmcouncil.org/fibo/LOAN/LoanTypes/CreditProducts/">
		<rdfs:label xml:lang="en">CreditProducts</rdfs:label>
		<dct:abstract>Terms specific to the existence and extension of credit. Includes terms like home equity lines of credit which may be referenced in asset backed securities. Also includes credit card facilities.</dct:abstract>
		<owl:imports rdf:resource="https://spec.edmcouncil.org/fibo/FBC/DebtAndEquities/CreditFacilities/"/>
		<owl:imports rdf:resource="https://spec.edmcouncil.org/fibo/FBC/DebtAndEquities/Debt/"/>
		<owl:imports rdf:resource="https://spec.edmcouncil.org/fibo/FND/Accounting/CurrencyAmount/"/>
		<owl:imports rdf:resource="https://spec.edmcouncil.org/fibo/FND/Utilities/AnnotationVocabulary/"/>
		<owl:imports rdf:resource="https://spec.edmcouncil.org/fibo/LOAN/Loans/LoansCollateral/"/>
		<owl:versionIRI rdf:resource="https://spec.edmcouncil.org/fibo/LOAN/LoanTypes/CreditProducts/"/>
		<fibo-fnd-utl-av:hasMaturityLevel rdf:resource="&fibo-fnd-utl-av;Provisional"/>
	</owl:Ontology>
	
	<owl:Class rdf:about="&fibo-loan-typ-cr;CreditCard">
		<rdfs:subClassOf rdf:resource="&fibo-fbc-dae-crf;CommittedCreditFacilityTranche"/>
		<rdfs:label xml:lang="en">credit card facility</rdfs:label>
	</owl:Class>
	
	<owl:Class rdf:about="&fibo-loan-typ-cr;HomeEquityLineOfCredit">
		<rdfs:subClassOf rdf:resource="&fibo-loan-typ-cr;RevolvingLineOfCredit"/>
		<rdfs:label xml:lang="en">home equity line of credit</rdfs:label>
		<skos:definition xml:lang="en">A credit line on a house or other property, that can be drawn down and/or paid back by the borrower.</skos:definition>
		<fibo-fnd-utl-av:explanatoryNote xml:lang="en">This is both a revolving line of credit and a mortgage, in that the collateral for the revolving line of credit in this case is some real estate, which is a defining fact for a mortgage. This form of product can either have an increase or decrease in principal, according to the actions of the borrower. These may also be used in the formation of asset pools for asset backed securities, though a specific named type of security has not been identified with these as underlying.</fibo-fnd-utl-av:explanatoryNote>
	</owl:Class>
	
	<owl:Class rdf:about="&fibo-loan-typ-cr;HomeEquityLineOfCreditContract">
		<rdfs:subClassOf rdf:resource="&fibo-loan-typ-cr;RevolvingCreditContract"/>
		<rdfs:subClassOf>
			<owl:Restriction>
				<owl:onProperty rdf:resource="&fibo-fbc-dae-crf;setsOutCommitmentTo"/>
				<owl:someValuesFrom rdf:resource="&fibo-loan-typ-cr;HomeEquityLineOfCreditTranche"/>
			</owl:Restriction>
		</rdfs:subClassOf>
		<rdfs:label xml:lang="en">home equity line of credit contract</rdfs:label>
		<skos:definition xml:lang="en">A credit line on a house or other property, that can be drawn down and/or paid back by the borrower.</skos:definition>
	</owl:Class>
	
	<owl:Class rdf:about="&fibo-loan-typ-cr;HomeEquityLineOfCreditTranche">
		<rdfs:subClassOf rdf:resource="&fibo-loan-typ-cr;RevolvingLineOfCreditTranche"/>
		<rdfs:subClassOf>
			<owl:Restriction>
				<owl:onProperty rdf:resource="&fibo-loan-typ-cr;becomesRevolvingLineOfCredit"/>
				<owl:someValuesFrom rdf:resource="&fibo-loan-typ-cr;HomeEquityLineOfCredit"/>
			</owl:Restriction>
		</rdfs:subClassOf>
		<rdfs:label xml:lang="en">home equity line of credit tranche</rdfs:label>
	</owl:Class>
	
	<owl:Class rdf:about="&fibo-loan-typ-cr;RevolvingCreditContract">
		<rdfs:subClassOf rdf:resource="&fibo-fbc-dae-crf;CreditFacilityAgreement"/>
		<rdfs:subClassOf>
			<owl:Restriction>
				<owl:onProperty rdf:resource="&fibo-fbc-dae-crf;setsOutCommitmentTo"/>
				<owl:someValuesFrom rdf:resource="&fibo-loan-typ-cr;RevolvingLineOfCreditTranche"/>
			</owl:Restriction>
		</rdfs:subClassOf>
		<rdfs:label xml:lang="en">revolving credit contract</rdfs:label>
		<skos:definition xml:lang="en">Contract which embodies and defines the terms and conditions for a credit line based on some collaterial, which can be drawn down and/or paid back by the borrower.</skos:definition>
	</owl:Class>
	
	<owl:Class rdf:about="&fibo-loan-typ-cr;RevolvingLineOfCredit">
		<rdfs:subClassOf rdf:resource="&fibo-fbc-dae-dbt;Debt"/>
		<rdfs:label xml:lang="en">revolving line of credit</rdfs:label>
		<skos:definition xml:lang="en">A credit line based on some collateral, that can be drawn down and/or paid back by the borrower.</skos:definition>
		<fibo-fnd-utl-av:explanatoryNote xml:lang="en">This form of product can either have an increase or decrease in principal, according to the actions of the borrower.</fibo-fnd-utl-av:explanatoryNote>
	</owl:Class>
	
	<owl:Class rdf:about="&fibo-loan-typ-cr;RevolvingLineOfCreditTranche">
		<rdfs:subClassOf rdf:resource="&fibo-fbc-dae-crf;CommittedCreditFacilityTranche"/>
		<rdfs:subClassOf>
			<owl:Restriction>
				<owl:onProperty rdf:resource="&fibo-loan-typ-cr;becomesRevolvingLineOfCredit"/>
				<owl:someValuesFrom rdf:resource="&fibo-loan-typ-cr;RevolvingLineOfCredit"/>
			</owl:Restriction>
		</rdfs:subClassOf>
		<rdfs:label xml:lang="en">revolving line of credit tranche</rdfs:label>
		<skos:definition xml:lang="en">A contractually committed line of credit which is issued as a revolving line of credit which can be drawn upon and has collateral</skos:definition>
	</owl:Class>
	
	<owl:ObjectProperty rdf:about="&fibo-loan-typ-cr;becomesRevolvingLineOfCredit">
		<rdfs:subPropertyOf rdf:resource="&fibo-fbc-dae-crf;issuedAs"/>
		<rdfs:label xml:lang="en">becomes revolving line of credit</rdfs:label>
		<rdfs:domain rdf:resource="&fibo-loan-typ-cr;RevolvingLineOfCreditTranche"/>
		<rdfs:range rdf:resource="&fibo-loan-typ-cr;RevolvingLineOfCredit"/>
	</owl:ObjectProperty>
	
	<owl:ObjectProperty rdf:about="&fibo-loan-typ-cr;maximumAllowedBalance">
		<rdfs:label xml:lang="en">maximum allowed balance  (please review)</rdfs:label>
		<rdfs:domain rdf:resource="&fibo-loan-typ-cr;RevolvingCreditContract"/>
		<rdfs:range rdf:resource="&fibo-fnd-acc-cur;MonetaryAmount"/>
		<skos:definition xml:lang="en">The maximum loan amount that is allowed to be outstanding as defined in this loan contract.</skos:definition>
	</owl:ObjectProperty>
	
	<owl:ObjectProperty rdf:about="&fibo-loan-typ-cr;maximumAnticipatedBalance">
		<rdfs:label xml:lang="en">maximum anticipated balance  (please review)</rdfs:label>
		<rdfs:domain rdf:resource="&fibo-loan-typ-cr;RevolvingLineOfCredit"/>
		<rdfs:range rdf:resource="&fibo-fnd-acc-cur;MonetaryAmount"/>
		<skos:definition xml:lang="en">The maximum loan amount that could potentially be outstanding.</skos:definition>
	</owl:ObjectProperty>

</rdf:RDF>