<?xml version="1.0" encoding="UTF-8"?>
  
<!DOCTYPE rdf:RDF [
    <!ENTITY fibo-sec-dbt-bond-bond "http://spec.edmcouncil.org/fibo/red/sec/debt/bonds/bonds-common/">
    <!ENTITY fibo-fnd-agr-ctr "http://spec.edmcouncil.org/fibo/red/fnd/agreements/contracts/">
    <!ENTITY fibo-sec-sec-cnv "http://spec.edmcouncil.org/fibo/red/sec/securities/securities-conversion-terms/">
    <!ENTITY fibo-sec-dbt-dbt-ins "http://spec.edmcouncil.org/fibo/red/sec/debt/debt-foundations/debt-instruments/">
    <!ENTITY fibo-sec-eq-eqi "http://spec.edmcouncil.org/fibo/red/sec/equities/equity-instruments/">
    <!ENTITY fibo-sec-dbt-bond-cfv "http://spec.edmcouncil.org/fibo/red/sec/debt/bonds/bonds-cashflow-variants/">
    <!ENTITY fibo-fnd-utl-bt "http://spec.edmcouncil.org/fibo/red/fnd/utilities/business-facing-types/">
    <!ENTITY fibo-sec-dbt-dbt-cfl "http://spec.edmcouncil.org/fibo/red/sec/debt/debt-foundations/debt-cashflow-terms/">
]>

<rdf:RDF xmlns:xsd="http://www.w3.org/2001/XMLSchema#"
         xmlns:sm="http://www.omg.org/techprocess/ab/SpecificationMetadata/"
         xmlns:xs="http://www.w3.org/2001/XMLSchema"
         xmlns:fibo-fnd-utl-av="http://www.omg.org/spec/EDMC-FIBO/FND/Utilities/AnnotationVocabulary/"
         xmlns:rdf="http://www.w3.org/1999/02/22-rdf-syntax-ns#"
         xmlns:rdfs="http://www.w3.org/2000/01/rdf-schema#"
         xmlns:owl="http://www.w3.org/2002/07/owl#"
         xmlns:skos="http://www.w3.org/2004/02/skos/core#"
         xmlns:dc="http://purl.org/dc/terms/"
         xml:base="http://spec.edmcouncil.org/fibo/red/sec/debt/bonds/bonds-common/">

   <owl:Ontology rdf:about="http://spec.edmcouncil.org/fibo/red/sec/debt/bonds/bonds-common/">
      <owl:imports rdf:resource="http://spec.edmcouncil.org/fibo/red/fnd/agreements/contracts/"/>
      <owl:imports rdf:resource="http://spec.edmcouncil.org/fibo/red/sec/securities/securities-conversion-terms/"/>
      <owl:imports rdf:resource="http://spec.edmcouncil.org/fibo/red/sec/debt/debt-foundations/debt-instruments/"/>
      <owl:imports rdf:resource="http://spec.edmcouncil.org/fibo/red/sec/equities/equity-instruments/"/>
      <owl:imports rdf:resource="http://spec.edmcouncil.org/fibo/red/sec/debt/bonds/bonds-cashflow-variants/"/>
      <owl:imports rdf:resource="http://spec.edmcouncil.org/fibo/red/fnd/utilities/business-facing-types/"/>
      <owl:imports rdf:resource="http://spec.edmcouncil.org/fibo/red/sec/debt/debt-foundations/debt-cashflow-terms/"/>
   </owl:Ontology>


  <!--
    ///////////////////////////////////////////////////////////////////////////////////////
    //
    // Datatypes
    //
    ///////////////////////////////////////////////////////////////////////////////////////
    -->



  <!--
    ///////////////////////////////////////////////////////////////////////////////////////
    //
    // Object Properties
    //
    ///////////////////////////////////////////////////////////////////////////////////////
    -->


<owl:ObjectProperty rdf:about="&fibo-sec-dbt-bond-bond;securitizationConditions.1">
      <rdfs:label>securitization conditions</rdfs:label>
      <rdfs:subPropertyOf rdf:resource="&fibo-fnd-agr-ctr;contractHasTerms"/>
      <rdfs:domain rdf:resource="&fibo-sec-dbt-bond-bond;Debenture"/>
      <rdfs:range rdf:resource="&fibo-sec-dbt-bond-bond;DebentureSecuritizationConditions"/>
   </owl:ObjectProperty>

   <owl:ObjectProperty rdf:about="&fibo-sec-dbt-bond-bond;convertibleInto">
      <rdfs:label>convertible into</rdfs:label>
      <rdfs:domain rdf:resource="&fibo-sec-dbt-bond-bond;ConvertibleBond"/>
      <rdfs:range rdf:resource="&fibo-sec-eq-eqi;PubliclyTradedShare"/>
   </owl:ObjectProperty>

   <owl:ObjectProperty rdf:about="&fibo-sec-dbt-bond-bond;hasConversionTerms">
      <rdfs:label>has conversion terms</rdfs:label>
      <rdfs:subPropertyOf rdf:resource="&fibo-fnd-agr-ctr;contractHasTerms"/>
      <rdfs:domain rdf:resource="&fibo-sec-dbt-bond-bond;ConvertibleBond"/>
      <rdfs:range rdf:resource="&fibo-sec-dbt-bond-bond;DebtConversionTermsSet"/>
   </owl:ObjectProperty>

   <owl:ObjectProperty rdf:about="&fibo-sec-dbt-bond-bond;specifiesConvertibleInto">
      <rdfs:label>specifies convertible into</rdfs:label>
      <rdfs:subPropertyOf rdf:resource="&fibo-sec-sec-cnv;specifiesConversionInto"/>
      <rdfs:domain rdf:resource="&fibo-sec-dbt-bond-bond;DebtConversionTermsSet"/>
      <rdfs:range rdf:resource="&fibo-sec-eq-eqi;PubliclyTradedShare"/>
   </owl:ObjectProperty>


  <!--
    ///////////////////////////////////////////////////////////////////////////////////////
    //
    // Data Properties
    //
    ///////////////////////////////////////////////////////////////////////////////////////
    -->


<owl:DatatypeProperty rdf:about="&fibo-sec-dbt-bond-bond;callable">
      <rdfs:label>callable</rdfs:label>
      <rdfs:range rdf:resource="&fibo-fnd-utl-bt;yesOrNo"/>
   </owl:DatatypeProperty>

   <owl:DatatypeProperty rdf:about="&fibo-sec-dbt-bond-bond;securitizationConditions">
      <rdfs:label>securitization conditions</rdfs:label>
      <skos:definition>Textual description of the conditions for the securitization of the Debenture.</skos:definition>
      <rdfs:range rdf:resource="&fibo-fnd-utl-bt;text"/>
   </owl:DatatypeProperty>

   <owl:DatatypeProperty rdf:about="&fibo-sec-dbt-bond-bond;convertibleDate">
      <rdfs:label>convertible date</rdfs:label>
      <skos:definition>Date on which the Bond can be converted into the specified Equity Security.</skos:definition>
      <rdfs:range rdf:resource="http://www.w3.org/2001/XMLSchema#date"/>
   </owl:DatatypeProperty>

   <owl:DatatypeProperty rdf:about="&fibo-sec-dbt-bond-bond;callable.1">
      <rdfs:label>callable</rdfs:label>
      <skos:definition>Whether the issuer has the right to pay the security prior to maturity.</skos:definition>
      <rdfs:range rdf:resource="&fibo-fnd-utl-bt;yesOrNo"/>
   </owl:DatatypeProperty>

   <owl:DatatypeProperty rdf:about="&fibo-sec-dbt-bond-bond;capitalizedInterest">
      <rdfs:label>capitalized interest</rdfs:label>
      <skos:definition>Whether the interest amount is capitalised until maturity date or paid out at each interest payment date.</skos:definition>
      <rdfs:range rdf:resource="&fibo-fnd-utl-bt;yesOrNo"/>
   </owl:DatatypeProperty>

   <owl:DatatypeProperty rdf:about="&fibo-sec-dbt-bond-bond;convertible">
      <rdfs:label>convertible</rdfs:label>
      <skos:definition>The bond has a conversion feature enabling it to be converted into another instrument on maturity.</skos:definition>
      <rdfs:range rdf:resource="&fibo-fnd-utl-bt;yesOrNo"/>
   </owl:DatatypeProperty>

   <owl:DatatypeProperty rdf:about="&fibo-sec-dbt-bond-bond;convertible.1">
      <rdfs:label>convertible</rdfs:label>
      <skos:definition>Bond is Convertible</skos:definition>
      <rdfs:range rdf:resource="&fibo-fnd-utl-bt;yesOrNo"/>
   </owl:DatatypeProperty>

   <owl:DatatypeProperty rdf:about="&fibo-sec-dbt-bond-bond;naked">
      <rdfs:label>naked</rdfs:label>
      <skos:definition>Whether the debenture is unsecured (Naked = Yes) or is secured (Naked = No).</skos:definition>
      <rdfs:range rdf:resource="&fibo-fnd-utl-bt;yesOrNo"/>
   </owl:DatatypeProperty>


  <!--
    ///////////////////////////////////////////////////////////////////////////////////////
    //
    // Annotation Properties
    //
    ///////////////////////////////////////////////////////////////////////////////////////
    -->



  <!--
    ///////////////////////////////////////////////////////////////////////////////////////
    //
    // Classes
    //
    ///////////////////////////////////////////////////////////////////////////////////////
    -->


<owl:Class rdf:about="&fibo-sec-dbt-bond-bond;BondWithPartialCall">
      <rdfs:label>bond with partial call</rdfs:label>
      <skos:definition>A bond with a feature whereby the issue can be partially called for amounts that are at the discretion of the issuer.</skos:definition>
      <rdfs:subClassOf rdf:resource="&fibo-sec-dbt-bond-bond;Bond"/>
   </owl:Class>

   <owl:Class rdf:about="&fibo-sec-dbt-bond-bond;CallableConvertibleBond">
      <rdfs:label>callable convertible bond</rdfs:label>
      <skos:definition>A Convertible Bond which is also callable.</skos:definition>
      <rdfs:subClassOf rdf:resource="&fibo-sec-dbt-bond-bond;ConvertibleBond"/>
   </owl:Class>

   <owl:Class rdf:about="&fibo-sec-dbt-bond-bond;DebentureSecuritizationConditions">
      <rdfs:label>debenture securitization conditions</rdfs:label>
      <skos:definition>Terms, if any, by which a Debenture is secured. This is a description of the properties by which it is secured, being those not otherwise pledged.</skos:definition>
      <rdfs:subClassOf rdf:resource="&fibo-fnd-agr-ctr;ContractTermsSet"/>
   </owl:Class>

   <owl:Class rdf:about="&fibo-sec-dbt-bond-bond;DebtConversionTermsSet">
      <rdfs:label>debt conversion terms set</rdfs:label>
      <skos:definition>Contractual specifications when a Convertible Bond can be converted to another security (usually of the same issuer).</skos:definition>
      <rdfs:subClassOf rdf:resource="&fibo-sec-dbt-dbt-cfl;TradableDebtSecurityRedemptionTermsSet"/>
      <rdfs:subClassOf rdf:resource="&fibo-sec-sec-cnv;ConversionTermsSet"/>
   </owl:Class>

   <owl:Class rdf:about="&fibo-sec-dbt-bond-bond;EquityLinkedBond">
      <rdfs:label>equity linked bond</rdfs:label>
      <skos:definition>A bond where the bond is based on the return on an equity over time i.e. the price and dividend payments i.e. the total return (similar to total return swaps).</skos:definition>
      <rdfs:subClassOf rdf:resource="&fibo-sec-dbt-bond-cfv;VariableCouponBond"/>
   </owl:Class>

   <owl:Class rdf:about="&fibo-sec-dbt-bond-bond;Bond">
      <rdfs:label>bond</rdfs:label>
      <skos:definition>A debt security, in which the authorized issuer owes the holders a debt and, depending on the terms of the bond, is obliged to pay interest (the coupon) and/or to repay the principal at a later date, termed maturity. It is a formal contract to repay borrowed money with interest at fixed intervals.</skos:definition>
      <rdfs:subClassOf rdf:resource="&fibo-sec-dbt-dbt-ins;TradableDebtInstrument"/>
   </owl:Class>

   <owl:Class rdf:about="&fibo-sec-dbt-bond-bond;BondWithWarrant">
      <rdfs:label>bond with warrant</rdfs:label>
      <skos:definition>A bond issue where the issue includes a Warrant attached. This need not be any specific type of bond.</skos:definition>
   </owl:Class>

   <owl:Class rdf:about="&fibo-sec-dbt-bond-bond;ConvertibleBond">
      <rdfs:label>convertible bond</rdfs:label>
      <skos:definition>A Bond instrument which on maturity converts into an Equity instrument.</skos:definition>
   </owl:Class>

   <owl:Class rdf:about="&fibo-sec-dbt-bond-bond;Debenture">
      <rdfs:label>debenture</rdfs:label>
      <skos:definition>A type of debt instrument that is not secured by physical asset or collateral. Debentures are backed only by the general creditworthiness and reputation of the issuer. Both corporations and governments frequently issue this type of bond in order to secure capital. Like other types of bonds, debentures are documented in an indenture.</skos:definition>
   </owl:Class>

   <owl:Class rdf:about="&fibo-sec-dbt-bond-bond;MediumTermNote">
      <rdfs:label>medium term note</rdfs:label>
      <skos:definition>A Medium Term Note is a Negotiable debt instrument offered under a program agreement through one or more dealers upon request of the Issuer. The Program defines the terms and conditions of the notes. An MTN issue is defined by the fact that the registration doesn't have a pre-defined maturity.</skos:definition>
   </owl:Class>


  <!--
    ///////////////////////////////////////////////////////////////////////////////////////
    //
    // Individuals
    //
    ///////////////////////////////////////////////////////////////////////////////////////
    -->


</rdf:RDF>